<?xml version="1.0"?>
<rdf:RDF xmlns="http://purl.obolibrary.org/obo/gaz/subsets/countries/Papua_New_Guinea.owl#"
     xml:base="http://purl.obolibrary.org/obo/gaz/subsets/countries/Papua_New_Guinea.owl"
     xmlns:obo="http://purl.obolibrary.org/obo/"
     xmlns:owl="http://www.w3.org/2002/07/owl#"
     xmlns:rdf="http://www.w3.org/1999/02/22-rdf-syntax-ns#"
     xmlns:xml="http://www.w3.org/XML/1998/namespace"
     xmlns:xsd="http://www.w3.org/2001/XMLSchema#"
     xmlns:rdfs="http://www.w3.org/2000/01/rdf-schema#"
     xmlns:oboInOwl="http://www.geneontology.org/formats/oboInOwl#">
    <owl:Ontology rdf:about="http://purl.obolibrary.org/obo/gaz/subsets/countries/Papua_New_Guinea.owl">
        <owl:imports rdf:resource="http://purl.obolibrary.org/obo/gaz/imports/envo_import.owl"/>
        <owl:imports rdf:resource="http://purl.obolibrary.org/obo/gaz/imports/ro_import.owl"/>
    </owl:Ontology>
    


    <!-- 
    ///////////////////////////////////////////////////////////////////////////////////////
    //
    // Annotation properties
    //
    ///////////////////////////////////////////////////////////////////////////////////////
     -->

    


    <!-- http://purl.obolibrary.org/obo/IAO_0000115 -->

    <owl:AnnotationProperty rdf:about="http://purl.obolibrary.org/obo/IAO_0000115"/>
    


    <!-- http://www.geneontology.org/formats/oboInOwl#hasOBONamespace -->

    <owl:AnnotationProperty rdf:about="http://www.geneontology.org/formats/oboInOwl#hasOBONamespace"/>
    


    <!-- http://www.geneontology.org/formats/oboInOwl#id -->

    <owl:AnnotationProperty rdf:about="http://www.geneontology.org/formats/oboInOwl#id"/>
    


    <!-- 
    ///////////////////////////////////////////////////////////////////////////////////////
    //
    // Object Properties
    //
    ///////////////////////////////////////////////////////////////////////////////////////
     -->

    


    <!-- http://purl.obolibrary.org/obo/RO_0001025 -->

    <owl:ObjectProperty rdf:about="http://purl.obolibrary.org/obo/RO_0001025"/>
    


    <!-- 
    ///////////////////////////////////////////////////////////////////////////////////////
    //
    // Classes
    //
    ///////////////////////////////////////////////////////////////////////////////////////
     -->

    


    <!-- http://purl.obolibrary.org/obo/ENVO_00000004 -->

    <owl:Class rdf:about="http://purl.obolibrary.org/obo/ENVO_00000004"/>
    


    <!-- http://purl.obolibrary.org/obo/ENVO_00000104 -->

    <owl:Class rdf:about="http://purl.obolibrary.org/obo/ENVO_00000104"/>
    


    <!-- http://purl.obolibrary.org/obo/ENVO_00000130 -->

    <owl:Class rdf:about="http://purl.obolibrary.org/obo/ENVO_00000130"/>
    


    <!-- http://purl.obolibrary.org/obo/ENVO_00000220 -->

    <owl:Class rdf:about="http://purl.obolibrary.org/obo/ENVO_00000220"/>
    


    <!-- http://purl.obolibrary.org/obo/ENVO_00000222 -->

    <owl:Class rdf:about="http://purl.obolibrary.org/obo/ENVO_00000222"/>
    


    <!-- http://purl.obolibrary.org/obo/ENVO_00000305 -->

    <owl:Class rdf:about="http://purl.obolibrary.org/obo/ENVO_00000305"/>
    


    <!-- http://purl.obolibrary.org/obo/ENVO_00000354 -->

    <owl:Class rdf:about="http://purl.obolibrary.org/obo/ENVO_00000354"/>
    


    <!-- http://purl.obolibrary.org/obo/GAZ_00005195 -->

    <owl:Class rdf:about="http://purl.obolibrary.org/obo/GAZ_00005195">
        <rdfs:subClassOf rdf:resource="http://purl.obolibrary.org/obo/GAZ_00005196"/>
    </owl:Class>
    


    <!-- http://purl.obolibrary.org/obo/GAZ_00005196 -->

    <owl:Class rdf:about="http://purl.obolibrary.org/obo/GAZ_00005196"/>
    


    <!-- http://purl.obolibrary.org/obo/GAZ_00005197 -->

    <owl:Class rdf:about="http://purl.obolibrary.org/obo/GAZ_00005197">
        <rdfs:subClassOf rdf:resource="http://purl.obolibrary.org/obo/GAZ_00005196"/>
    </owl:Class>
    


    <!-- http://purl.obolibrary.org/obo/GAZ_00005199 -->

    <owl:Class rdf:about="http://purl.obolibrary.org/obo/GAZ_00005199">
        <rdfs:subClassOf rdf:resource="http://purl.obolibrary.org/obo/GAZ_00005196"/>
    </owl:Class>
    


    <!-- http://purl.obolibrary.org/obo/GAZ_00005205 -->

    <owl:Class rdf:about="http://purl.obolibrary.org/obo/GAZ_00005205">
        <rdfs:subClassOf rdf:resource="http://purl.obolibrary.org/obo/GAZ_00005196"/>
    </owl:Class>
    


    <!-- http://purl.obolibrary.org/obo/GAZ_00005217 -->

    <owl:Class rdf:about="http://purl.obolibrary.org/obo/GAZ_00005217">
        <rdfs:subClassOf rdf:resource="http://purl.obolibrary.org/obo/GAZ_00005196"/>
    </owl:Class>
    


    <!-- http://purl.obolibrary.org/obo/GAZ_00005263 -->

    <owl:Class rdf:about="http://purl.obolibrary.org/obo/GAZ_00005263">
        <rdfs:subClassOf rdf:resource="http://purl.obolibrary.org/obo/GAZ_00005196"/>
    </owl:Class>
    


    <!-- http://purl.obolibrary.org/obo/GAZ_00005267 -->

    <owl:Class rdf:about="http://purl.obolibrary.org/obo/GAZ_00005267">
        <rdfs:subClassOf rdf:resource="http://purl.obolibrary.org/obo/GAZ_00005196"/>
    </owl:Class>
    


    <!-- http://purl.obolibrary.org/obo/GAZ_00007257 -->

    <owl:Class rdf:about="http://purl.obolibrary.org/obo/GAZ_00007257">
        <rdfs:subClassOf rdf:resource="http://purl.obolibrary.org/obo/GAZ_00005196"/>
    </owl:Class>
    


    <!-- http://purl.obolibrary.org/obo/GAZ_00010065 -->

    <owl:Class rdf:about="http://purl.obolibrary.org/obo/GAZ_00010065">
        <rdfs:subClassOf rdf:resource="http://purl.obolibrary.org/obo/GAZ_00005196"/>
    </owl:Class>
    


    <!-- http://purl.obolibrary.org/obo/GAZ_00016819 -->

    <owl:Class rdf:about="http://purl.obolibrary.org/obo/GAZ_00016819"/>
    


    <!-- http://purl.obolibrary.org/obo/GAZ_00117917 -->

    <owl:Class rdf:about="http://purl.obolibrary.org/obo/GAZ_00117917"/>
    


    <!-- http://purl.obolibrary.org/obo/GAZ_00117918 -->

    <owl:Class rdf:about="http://purl.obolibrary.org/obo/GAZ_00117918">
        <rdfs:subClassOf rdf:resource="http://purl.obolibrary.org/obo/GAZ_00117917"/>
    </owl:Class>
    


    <!-- http://purl.obolibrary.org/obo/GAZ_00117919 -->

    <owl:Class rdf:about="http://purl.obolibrary.org/obo/GAZ_00117919">
        <rdfs:subClassOf rdf:resource="http://purl.obolibrary.org/obo/GAZ_00117917"/>
    </owl:Class>
    


    <!-- http://purl.obolibrary.org/obo/GAZ_00117920 -->

    <owl:Class rdf:about="http://purl.obolibrary.org/obo/GAZ_00117920">
        <rdfs:subClassOf rdf:resource="http://purl.obolibrary.org/obo/GAZ_00117917"/>
    </owl:Class>
    


    <!-- http://purl.obolibrary.org/obo/GAZ_00117921 -->

    <owl:Class rdf:about="http://purl.obolibrary.org/obo/GAZ_00117921">
        <rdfs:subClassOf rdf:resource="http://purl.obolibrary.org/obo/GAZ_00117917"/>
    </owl:Class>
    


    <!-- http://purl.obolibrary.org/obo/GAZ_00253640 -->

    <owl:Class rdf:about="http://purl.obolibrary.org/obo/GAZ_00253640"/>
    


    <!-- http://purl.obolibrary.org/obo/GAZ_00253641 -->

    <owl:Class rdf:about="http://purl.obolibrary.org/obo/GAZ_00253641">
        <rdfs:subClassOf rdf:resource="http://purl.obolibrary.org/obo/GAZ_00253640"/>
        <obo:IAO_0000115>A cave.</obo:IAO_0000115>
        <oboInOwl:hasOBONamespace>GAZ</oboInOwl:hasOBONamespace>
        <oboInOwl:id>GAZ:00253641</oboInOwl:id>
        <rdfs:label>Triosaurus Cave</rdfs:label>
    </owl:Class>
    


    <!-- http://purl.obolibrary.org/obo/GAZ_00253930 -->

    <owl:Class rdf:about="http://purl.obolibrary.org/obo/GAZ_00253930">
        <rdfs:subClassOf rdf:resource="http://purl.obolibrary.org/obo/GAZ_00016819"/>
        <obo:IAO_0000115>A protected area.</obo:IAO_0000115>
        <oboInOwl:hasOBONamespace>GAZ</oboInOwl:hasOBONamespace>
        <oboInOwl:id>GAZ:00253930</oboInOwl:id>
        <rdfs:label>Ndrolowa Wildlife Management Area</rdfs:label>
    </owl:Class>
    


    <!-- 
    ///////////////////////////////////////////////////////////////////////////////////////
    //
    // Individuals
    //
    ///////////////////////////////////////////////////////////////////////////////////////
     -->

    


    <!-- http://purl.obolibrary.org/obo/GAZ_00003922 -->

    <owl:NamedIndividual rdf:about="http://purl.obolibrary.org/obo/GAZ_00003922">
        <oboInOwl:hasOBONamespace>GAZ</oboInOwl:hasOBONamespace>
        <oboInOwl:id>GAZ:00003922</oboInOwl:id>
        <rdfs:label>Papua New Guinea</rdfs:label>
    </owl:NamedIndividual>
    


    <!-- http://purl.obolibrary.org/obo/GAZ_00005182 -->

    <owl:NamedIndividual rdf:about="http://purl.obolibrary.org/obo/GAZ_00005182">
        <obo:RO_0001025 rdf:resource="http://purl.obolibrary.org/obo/GAZ_00117920"/>
        <obo:IAO_0000115>An autonomous region in Papua New Guinea and is the largest of the Solomon Islands group.</obo:IAO_0000115>
        <oboInOwl:hasOBONamespace>GAZ</oboInOwl:hasOBONamespace>
        <oboInOwl:id>GAZ:00005182</oboInOwl:id>
        <rdfs:label>North Solomons Province</rdfs:label>
    </owl:NamedIndividual>
    


    <!-- http://purl.obolibrary.org/obo/GAZ_00005184 -->

    <owl:NamedIndividual rdf:about="http://purl.obolibrary.org/obo/GAZ_00005184">
        <obo:RO_0001025 rdf:resource="http://purl.obolibrary.org/obo/GAZ_00005182"/>
        <obo:IAO_0000115>The largest island of the Solomon Islands group, politically part of Papua New Guinea.</obo:IAO_0000115>
        <oboInOwl:hasOBONamespace>GAZ</oboInOwl:hasOBONamespace>
        <oboInOwl:id>GAZ:00005184</oboInOwl:id>
        <rdfs:label>Bougainville Island</rdfs:label>
    </owl:NamedIndividual>
    


    <!-- http://purl.obolibrary.org/obo/GAZ_00005185 -->

    <owl:NamedIndividual rdf:about="http://purl.obolibrary.org/obo/GAZ_00005185">
        <obo:RO_0001025 rdf:resource="http://purl.obolibrary.org/obo/GAZ_00005186"/>
        <oboInOwl:hasOBONamespace>GAZ</oboInOwl:hasOBONamespace>
        <oboInOwl:id>GAZ:00005185</oboInOwl:id>
        <rdfs:label>Piul Island</rdfs:label>
    </owl:NamedIndividual>
    


    <!-- http://purl.obolibrary.org/obo/GAZ_00005186 -->

    <owl:NamedIndividual rdf:about="http://purl.obolibrary.org/obo/GAZ_00005186">
        <obo:RO_0001025 rdf:resource="http://purl.obolibrary.org/obo/GAZ_00118095"/>
        <obo:IAO_0000115>An atoll located 86 km north-east of Bougainville in the South Pacific. The atoll is a scattering of low lying islands in a horseshoe shape stretching 30 km in north-south direction, with a total land area of 0.6 km2 and a maximum elevation of 1.5 m above sea level.</obo:IAO_0000115>
        <oboInOwl:hasOBONamespace>GAZ</oboInOwl:hasOBONamespace>
        <oboInOwl:id>GAZ:00005186</oboInOwl:id>
        <rdfs:label>Carteret Islands</rdfs:label>
    </owl:NamedIndividual>
    


    <!-- http://purl.obolibrary.org/obo/GAZ_00005188 -->

    <owl:NamedIndividual rdf:about="http://purl.obolibrary.org/obo/GAZ_00005188">
        <obo:RO_0001025 rdf:resource="http://purl.obolibrary.org/obo/GAZ_00005190"/>
        <obo:RO_0001025 rdf:resource="http://purl.obolibrary.org/obo/GAZ_00022398"/>
        <obo:IAO_0000115>A large island in Papua New Guinea, approximately 8,650 km2 in area. It is the main and largest island of the New Ireland Province. It lies northeast of the island of New Britain. Both islands are a part of the Bismarck Archipelago and are separated by the Saint George&apos;s Channel.</obo:IAO_0000115>
        <oboInOwl:hasOBONamespace>GAZ</oboInOwl:hasOBONamespace>
        <oboInOwl:id>GAZ:00005188</oboInOwl:id>
        <rdfs:label>New Ireland</rdfs:label>
    </owl:NamedIndividual>
    


    <!-- http://purl.obolibrary.org/obo/GAZ_00005189 -->

    <owl:NamedIndividual rdf:about="http://purl.obolibrary.org/obo/GAZ_00005189">
        <obo:RO_0001025 rdf:resource="http://purl.obolibrary.org/obo/GAZ_00005193"/>
        <obo:IAO_0000115>The largest island in the Bismarck Archipelago of Papua New Guinea, separated from the island of New Guinea by Dampier Strait.</obo:IAO_0000115>
        <oboInOwl:hasOBONamespace>GAZ</oboInOwl:hasOBONamespace>
        <oboInOwl:id>GAZ:00005189</oboInOwl:id>
        <rdfs:label>New Britain</rdfs:label>
    </owl:NamedIndividual>
    


    <!-- http://purl.obolibrary.org/obo/GAZ_00005190 -->

    <owl:NamedIndividual rdf:about="http://purl.obolibrary.org/obo/GAZ_00005190">
        <obo:RO_0001025 rdf:resource="http://purl.obolibrary.org/obo/GAZ_00117920"/>
        <obo:IAO_0000115>The most northeastern province of Papua New Guinea.</obo:IAO_0000115>
        <oboInOwl:hasOBONamespace>GAZ</oboInOwl:hasOBONamespace>
        <oboInOwl:id>GAZ:00005190</oboInOwl:id>
        <rdfs:label>New Ireland Province</rdfs:label>
    </owl:NamedIndividual>
    


    <!-- http://purl.obolibrary.org/obo/GAZ_00005191 -->

    <owl:NamedIndividual rdf:about="http://purl.obolibrary.org/obo/GAZ_00005191">
        <rdf:type rdf:resource="http://purl.obolibrary.org/obo/ENVO_00000104"/>
        <obo:RO_0001025 rdf:resource="http://purl.obolibrary.org/obo/GAZ_00117920"/>
        <obo:IAO_0000115>A province of Papua New Guinea on the islands of New Britain. The provincial capital is Kimbe.</obo:IAO_0000115>
        <oboInOwl:hasOBONamespace>GAZ</oboInOwl:hasOBONamespace>
        <oboInOwl:id>GAZ:00005191</oboInOwl:id>
        <rdfs:label>West New Britain Province</rdfs:label>
    </owl:NamedIndividual>
    


    <!-- http://purl.obolibrary.org/obo/GAZ_00005192 -->

    <owl:NamedIndividual rdf:about="http://purl.obolibrary.org/obo/GAZ_00005192">
        <rdf:type rdf:resource="http://purl.obolibrary.org/obo/ENVO_00000104"/>
        <obo:RO_0001025 rdf:resource="http://purl.obolibrary.org/obo/GAZ_00117920"/>
        <obo:IAO_0000115>A province of Papua New Guinea, on the island of New Britain. The capital of the province is Kokopo, not far from the old capital of Rabaul, which was largely destroyed in a 1994 volcanic eruption.</obo:IAO_0000115>
        <oboInOwl:hasOBONamespace>GAZ</oboInOwl:hasOBONamespace>
        <oboInOwl:id>GAZ:00005192</oboInOwl:id>
        <rdfs:label>East New Britain Province</rdfs:label>
    </owl:NamedIndividual>
    


    <!-- http://purl.obolibrary.org/obo/GAZ_00005193 -->

    <owl:NamedIndividual rdf:about="http://purl.obolibrary.org/obo/GAZ_00005193">
        <obo:RO_0001025 rdf:resource="http://purl.obolibrary.org/obo/GAZ_00003922"/>
        <obo:IAO_0000115>A group of mostly volcanic islands off the northeastern coast of New Guinea in the western Pacific Ocean and part of Papua New Guinea.</obo:IAO_0000115>
        <oboInOwl:hasOBONamespace>GAZ</oboInOwl:hasOBONamespace>
        <oboInOwl:id>GAZ:00005193</oboInOwl:id>
        <rdfs:label>Bismarck Archipelago</rdfs:label>
    </owl:NamedIndividual>
    


    <!-- http://purl.obolibrary.org/obo/GAZ_00005194 -->

    <owl:NamedIndividual rdf:about="http://purl.obolibrary.org/obo/GAZ_00005194">
        <obo:RO_0001025 rdf:resource="http://purl.obolibrary.org/obo/GAZ_00005195"/>
        <oboInOwl:hasOBONamespace>GAZ</oboInOwl:hasOBONamespace>
        <oboInOwl:id>GAZ:00005194</oboInOwl:id>
        <rdfs:label>Aropa Airstrip</rdfs:label>
    </owl:NamedIndividual>
    


    <!-- http://purl.obolibrary.org/obo/GAZ_00005195 -->

    <owl:NamedIndividual rdf:about="http://purl.obolibrary.org/obo/GAZ_00005195">
        <obo:RO_0001025 rdf:resource="http://purl.obolibrary.org/obo/GAZ_00022404"/>
    </owl:NamedIndividual>
    


    <!-- http://purl.obolibrary.org/obo/GAZ_00005196 -->

    <owl:NamedIndividual rdf:about="http://purl.obolibrary.org/obo/GAZ_00005196">
        <obo:RO_0001025 rdf:resource="http://purl.obolibrary.org/obo/GAZ_00003922"/>
    </owl:NamedIndividual>
    


    <!-- http://purl.obolibrary.org/obo/GAZ_00005197 -->

    <owl:NamedIndividual rdf:about="http://purl.obolibrary.org/obo/GAZ_00005197">
        <obo:RO_0001025 rdf:resource="http://purl.obolibrary.org/obo/GAZ_00022406"/>
    </owl:NamedIndividual>
    


    <!-- http://purl.obolibrary.org/obo/GAZ_00005198 -->

    <owl:NamedIndividual rdf:about="http://purl.obolibrary.org/obo/GAZ_00005198">
        <rdf:type rdf:resource="http://purl.obolibrary.org/obo/ENVO_00000104"/>
        <obo:RO_0001025 rdf:resource="http://purl.obolibrary.org/obo/GAZ_00117919"/>
        <obo:IAO_0000115>A province on the northern coast of mainland Papua New Guinea.</obo:IAO_0000115>
        <oboInOwl:hasOBONamespace>GAZ</oboInOwl:hasOBONamespace>
        <oboInOwl:id>GAZ:00005198</oboInOwl:id>
        <rdfs:label>Madang Province</rdfs:label>
    </owl:NamedIndividual>
    


    <!-- http://purl.obolibrary.org/obo/GAZ_00005199 -->

    <owl:NamedIndividual rdf:about="http://purl.obolibrary.org/obo/GAZ_00005199">
        <obo:RO_0001025 rdf:resource="http://purl.obolibrary.org/obo/GAZ_00005198"/>
    </owl:NamedIndividual>
    


    <!-- http://purl.obolibrary.org/obo/GAZ_00005202 -->

    <owl:NamedIndividual rdf:about="http://purl.obolibrary.org/obo/GAZ_00005202">
        <obo:RO_0001025 rdf:resource="http://purl.obolibrary.org/obo/GAZ_00005198"/>
        <oboInOwl:hasOBONamespace>GAZ</oboInOwl:hasOBONamespace>
        <oboInOwl:id>GAZ:00005202</oboInOwl:id>
        <rdfs:label>Balek Wildlife Sanctuary</rdfs:label>
    </owl:NamedIndividual>
    


    <!-- http://purl.obolibrary.org/obo/GAZ_00005203 -->

    <owl:NamedIndividual rdf:about="http://purl.obolibrary.org/obo/GAZ_00005203">
        <obo:RO_0001025 rdf:resource="http://purl.obolibrary.org/obo/GAZ_00005198"/>
        <oboInOwl:hasOBONamespace>GAZ</oboInOwl:hasOBONamespace>
        <oboInOwl:id>GAZ:00005203</oboInOwl:id>
        <rdfs:label>Hansa Bay</rdfs:label>
    </owl:NamedIndividual>
    


    <!-- http://purl.obolibrary.org/obo/GAZ_00005204 -->

    <owl:NamedIndividual rdf:about="http://purl.obolibrary.org/obo/GAZ_00005204">
        <obo:RO_0001025 rdf:resource="http://purl.obolibrary.org/obo/GAZ_00005203"/>
        <oboInOwl:hasOBONamespace>GAZ</oboInOwl:hasOBONamespace>
        <oboInOwl:id>GAZ:00005204</oboInOwl:id>
        <rdfs:label>Laing Island</rdfs:label>
    </owl:NamedIndividual>
    


    <!-- http://purl.obolibrary.org/obo/GAZ_00005205 -->

    <owl:NamedIndividual rdf:about="http://purl.obolibrary.org/obo/GAZ_00005205">
        <obo:RO_0001025 rdf:resource="http://purl.obolibrary.org/obo/GAZ_00005198"/>
    </owl:NamedIndividual>
    


    <!-- http://purl.obolibrary.org/obo/GAZ_00005217 -->

    <owl:NamedIndividual rdf:about="http://purl.obolibrary.org/obo/GAZ_00005217">
        <obo:RO_0001025 rdf:resource="http://purl.obolibrary.org/obo/GAZ_00022377"/>
    </owl:NamedIndividual>
    


    <!-- http://purl.obolibrary.org/obo/GAZ_00005263 -->

    <owl:NamedIndividual rdf:about="http://purl.obolibrary.org/obo/GAZ_00005263">
        <obo:RO_0001025 rdf:resource="http://purl.obolibrary.org/obo/GAZ_00005264"/>
    </owl:NamedIndividual>
    


    <!-- http://purl.obolibrary.org/obo/GAZ_00005264 -->

    <owl:NamedIndividual rdf:about="http://purl.obolibrary.org/obo/GAZ_00005264">
        <obo:RO_0001025 rdf:resource="http://purl.obolibrary.org/obo/GAZ_00117921"/>
        <obo:IAO_0000115>The incorporated area around Port Moresby, which is the capital of Papua New Guinea. It is surrounded by Central Province, where Port Moresby is also the capital, it is technically not a part of that province.</obo:IAO_0000115>
        <oboInOwl:hasOBONamespace>GAZ</oboInOwl:hasOBONamespace>
        <oboInOwl:id>GAZ:00005264</oboInOwl:id>
        <rdfs:label>National Capital District</rdfs:label>
    </owl:NamedIndividual>
    


    <!-- http://purl.obolibrary.org/obo/GAZ_00005266 -->

    <owl:NamedIndividual rdf:about="http://purl.obolibrary.org/obo/GAZ_00005266">
        <rdf:type rdf:resource="http://purl.obolibrary.org/obo/ENVO_00000104"/>
        <obo:RO_0001025 rdf:resource="http://purl.obolibrary.org/obo/GAZ_00117919"/>
        <obo:IAO_0000115>A province in Papua New Guinea. Its capital is Wewak.</obo:IAO_0000115>
        <oboInOwl:hasOBONamespace>GAZ</oboInOwl:hasOBONamespace>
        <oboInOwl:id>GAZ:00005266</oboInOwl:id>
        <rdfs:label>East Sepik Province</rdfs:label>
    </owl:NamedIndividual>
    


    <!-- http://purl.obolibrary.org/obo/GAZ_00005267 -->

    <owl:NamedIndividual rdf:about="http://purl.obolibrary.org/obo/GAZ_00005267">
        <obo:RO_0001025 rdf:resource="http://purl.obolibrary.org/obo/GAZ_00022370"/>
    </owl:NamedIndividual>
    


    <!-- http://purl.obolibrary.org/obo/GAZ_00007179 -->

    <owl:NamedIndividual rdf:about="http://purl.obolibrary.org/obo/GAZ_00007179">
        <obo:RO_0001025 rdf:resource="http://purl.obolibrary.org/obo/GAZ_00005193"/>
        <obo:RO_0001025 rdf:resource="http://purl.obolibrary.org/obo/GAZ_00022378"/>
        <obo:IAO_0000115>A group of 18 islands in the Bismarck Archipelago. The islands form part of Manus Province of Papua New Guinea.</obo:IAO_0000115>
        <oboInOwl:hasOBONamespace>GAZ</oboInOwl:hasOBONamespace>
        <oboInOwl:id>GAZ:00007179</oboInOwl:id>
        <rdfs:label>Admiralty Islands</rdfs:label>
    </owl:NamedIndividual>
    


    <!-- http://purl.obolibrary.org/obo/GAZ_00007180 -->

    <owl:NamedIndividual rdf:about="http://purl.obolibrary.org/obo/GAZ_00007180">
        <obo:RO_0001025 rdf:resource="http://purl.obolibrary.org/obo/GAZ_00022398"/>
        <obo:RO_0001025 rdf:resource="http://purl.obolibrary.org/obo/GAZ_00118104"/>
        <obo:IAO_0000115>A small group of islands in the Bismarck Archipelago, that makes up part of Papua New Guinea.</obo:IAO_0000115>
        <oboInOwl:hasOBONamespace>GAZ</oboInOwl:hasOBONamespace>
        <oboInOwl:id>GAZ:00007180</oboInOwl:id>
        <rdfs:label>Saint Matthias Islands</rdfs:label>
    </owl:NamedIndividual>
    


    <!-- http://purl.obolibrary.org/obo/GAZ_00007181 -->

    <owl:NamedIndividual rdf:about="http://purl.obolibrary.org/obo/GAZ_00007181">
        <obo:RO_0001025 rdf:resource="http://purl.obolibrary.org/obo/GAZ_00012666"/>
        <obo:RO_0001025 rdf:resource="http://purl.obolibrary.org/obo/GAZ_00051599"/>
        <obo:IAO_0000115>A group of islands near the eastern tip of New Guinea in the Solomon Sea in Milne Bay Province of Papua New Guinea. The group spans a distance of 160 km, has a total land area of approximately 3,100 km2 and is separated from the Papua New Guinea mainland by the 30 km wide Ward Hunt Strait in the north and the 18 km wide Goschen Strait in the south. D&apos;Entrecasteaux Islands show signs of vulcanism.</obo:IAO_0000115>
        <oboInOwl:hasOBONamespace>GAZ</oboInOwl:hasOBONamespace>
        <oboInOwl:id>GAZ:00007181</oboInOwl:id>
        <rdfs:label>D&apos;Entrecasteaux Islands</rdfs:label>
    </owl:NamedIndividual>
    


    <!-- http://purl.obolibrary.org/obo/GAZ_00007182 -->

    <owl:NamedIndividual rdf:about="http://purl.obolibrary.org/obo/GAZ_00007182">
        <obo:RO_0001025 rdf:resource="http://purl.obolibrary.org/obo/GAZ_00051599"/>
        <obo:RO_0001025 rdf:resource="http://purl.obolibrary.org/obo/GAZ_00118045"/>
        <obo:IAO_0000115>A string of ten volcanic islands and coral reefs located just southeast of New Guinea, between the Solomon Sea to the north and the Coral Sea to the south. Sideia Island and Basilaki Island lie closest to New Guinea, while Misima, Vanatinai (called Sudest or Tagula as named by European claimants on Western maps), and Rossel islands lie further east.</obo:IAO_0000115>
        <oboInOwl:hasOBONamespace>GAZ</oboInOwl:hasOBONamespace>
        <oboInOwl:id>GAZ:00007182</oboInOwl:id>
        <rdfs:label>Louisiade Archipelago</rdfs:label>
    </owl:NamedIndividual>
    


    <!-- http://purl.obolibrary.org/obo/GAZ_00007183 -->

    <owl:NamedIndividual rdf:about="http://purl.obolibrary.org/obo/GAZ_00007183">
        <obo:RO_0001025 rdf:resource="http://purl.obolibrary.org/obo/GAZ_00022382"/>
        <obo:RO_0001025 rdf:resource="http://purl.obolibrary.org/obo/GAZ_00051599"/>
        <obo:IAO_0000115>A 170 mi2 archipelago of coral atolls off the eastern coast of New Guinea. They are situated in Milne Bay Province in Papua New Guinea.</obo:IAO_0000115>
        <oboInOwl:hasOBONamespace>GAZ</oboInOwl:hasOBONamespace>
        <oboInOwl:id>GAZ:00007183</oboInOwl:id>
        <rdfs:label>Trobriand Islands</rdfs:label>
    </owl:NamedIndividual>
    


    <!-- http://purl.obolibrary.org/obo/GAZ_00007200 -->

    <owl:NamedIndividual rdf:about="http://purl.obolibrary.org/obo/GAZ_00007200">
        <obo:RO_0001025 rdf:resource="http://purl.obolibrary.org/obo/GAZ_00118095"/>
        <obo:IAO_0000115>A group of islands. Located nearly 200 km northeast of New Ireland and 126 km from the Tabar-Lihir-Tanga-Feni island arc, the Nuguria Islands consist of two closely spaced atoll formations.</obo:IAO_0000115>
        <oboInOwl:hasOBONamespace>GAZ</oboInOwl:hasOBONamespace>
        <oboInOwl:id>GAZ:00007200</oboInOwl:id>
        <rdfs:label>Nuguria Islands</rdfs:label>
    </owl:NamedIndividual>
    


    <!-- http://purl.obolibrary.org/obo/GAZ_00007201 -->

    <owl:NamedIndividual rdf:about="http://purl.obolibrary.org/obo/GAZ_00007201">
        <obo:RO_0001025 rdf:resource="http://purl.obolibrary.org/obo/GAZ_00118095"/>
        <obo:IAO_0000115>A ring of more than twenty islets on a reef surrounding a large lagoon. They are located on a sandy strip of coral no more than a meter above sea level just 4 degrees south of the equator.</obo:IAO_0000115>
        <oboInOwl:hasOBONamespace>GAZ</oboInOwl:hasOBONamespace>
        <oboInOwl:id>GAZ:00007201</oboInOwl:id>
        <rdfs:label>Nukumanu Islands</rdfs:label>
    </owl:NamedIndividual>
    


    <!-- http://purl.obolibrary.org/obo/GAZ_00007209 -->

    <owl:NamedIndividual rdf:about="http://purl.obolibrary.org/obo/GAZ_00007209">
        <obo:RO_0001025 rdf:resource="http://purl.obolibrary.org/obo/GAZ_00118095"/>
        <obo:IAO_0000115>A small, isolated atoll off the east coast of Bougainville in Papua New Guinea. Takuu lies about 250 km to the northeast of Kieta, capital of Bougainville, at the intersection of two shifting tectonic plates, which are causing the atoll to sink. The atoll consists of about 13 islands to the east and one island to the northwest.</obo:IAO_0000115>
        <oboInOwl:hasOBONamespace>GAZ</oboInOwl:hasOBONamespace>
        <oboInOwl:id>GAZ:00007209</oboInOwl:id>
        <rdfs:label>Takuu Island</rdfs:label>
    </owl:NamedIndividual>
    


    <!-- http://purl.obolibrary.org/obo/GAZ_00007255 -->

    <owl:NamedIndividual rdf:about="http://purl.obolibrary.org/obo/GAZ_00007255">
        <rdf:type rdf:resource="http://purl.obolibrary.org/obo/ENVO_00000104"/>
        <obo:RO_0001025 rdf:resource="http://purl.obolibrary.org/obo/GAZ_00117919"/>
        <obo:IAO_0000115>A province on the northern coast of Papua New Guinea.</obo:IAO_0000115>
        <oboInOwl:hasOBONamespace>GAZ</oboInOwl:hasOBONamespace>
        <oboInOwl:id>GAZ:00007255</oboInOwl:id>
        <rdfs:label>Morobe Province</rdfs:label>
    </owl:NamedIndividual>
    


    <!-- http://purl.obolibrary.org/obo/GAZ_00007256 -->

    <owl:NamedIndividual rdf:about="http://purl.obolibrary.org/obo/GAZ_00007256">
        <rdf:type rdf:resource="http://purl.obolibrary.org/obo/ENVO_00000004"/>
        <obo:RO_0001025 rdf:resource="http://purl.obolibrary.org/obo/GAZ_00007255"/>
        <obo:IAO_0000115>A district of Morobe Province, Papua New Guinea.</obo:IAO_0000115>
        <oboInOwl:hasOBONamespace>GAZ</oboInOwl:hasOBONamespace>
        <oboInOwl:id>GAZ:00007256</oboInOwl:id>
        <rdfs:label>Finschhafen District</rdfs:label>
    </owl:NamedIndividual>
    


    <!-- http://purl.obolibrary.org/obo/GAZ_00007257 -->

    <owl:NamedIndividual rdf:about="http://purl.obolibrary.org/obo/GAZ_00007257">
        <obo:RO_0001025 rdf:resource="http://purl.obolibrary.org/obo/GAZ_00022387"/>
    </owl:NamedIndividual>
    


    <!-- http://purl.obolibrary.org/obo/GAZ_00008618 -->

    <owl:NamedIndividual rdf:about="http://purl.obolibrary.org/obo/GAZ_00008618">
        <obo:RO_0001025 rdf:resource="http://purl.obolibrary.org/obo/GAZ_00005217"/>
        <oboInOwl:hasOBONamespace>GAZ</oboInOwl:hasOBONamespace>
        <oboInOwl:id>GAZ:00008618</oboInOwl:id>
        <rdfs:label>Matupi Harbor</rdfs:label>
    </owl:NamedIndividual>
    


    <!-- http://purl.obolibrary.org/obo/GAZ_00010064 -->

    <owl:NamedIndividual rdf:about="http://purl.obolibrary.org/obo/GAZ_00010064">
        <obo:RO_0001025 rdf:resource="http://purl.obolibrary.org/obo/GAZ_00117918"/>
        <oboInOwl:hasOBONamespace>GAZ</oboInOwl:hasOBONamespace>
        <oboInOwl:id>GAZ:00010064</oboInOwl:id>
        <rdfs:label>Eastern Highlands Province</rdfs:label>
    </owl:NamedIndividual>
    


    <!-- http://purl.obolibrary.org/obo/GAZ_00010065 -->

    <owl:NamedIndividual rdf:about="http://purl.obolibrary.org/obo/GAZ_00010065">
        <obo:RO_0001025 rdf:resource="http://purl.obolibrary.org/obo/GAZ_00022368"/>
    </owl:NamedIndividual>
    


    <!-- http://purl.obolibrary.org/obo/GAZ_00012657 -->

    <owl:NamedIndividual rdf:about="http://purl.obolibrary.org/obo/GAZ_00012657">
        <rdf:type rdf:resource="http://purl.obolibrary.org/obo/ENVO_00000104"/>
        <obo:RO_0001025 rdf:resource="http://purl.obolibrary.org/obo/GAZ_00117921"/>
        <obo:IAO_0000115>A province in Papua New Guinea located on the southern coast of the country.</obo:IAO_0000115>
        <oboInOwl:hasOBONamespace>GAZ</oboInOwl:hasOBONamespace>
        <oboInOwl:id>GAZ:00012657</oboInOwl:id>
        <rdfs:label>Central Province</rdfs:label>
    </owl:NamedIndividual>
    


    <!-- http://purl.obolibrary.org/obo/GAZ_00012658 -->

    <owl:NamedIndividual rdf:about="http://purl.obolibrary.org/obo/GAZ_00012658">
        <rdf:type rdf:resource="http://purl.obolibrary.org/obo/ENVO_00000104"/>
        <obo:RO_0001025 rdf:resource="http://purl.obolibrary.org/obo/GAZ_00117918"/>
        <obo:IAO_0000115>A Highlands Region province in Papua New Guinea.</obo:IAO_0000115>
        <oboInOwl:hasOBONamespace>GAZ</oboInOwl:hasOBONamespace>
        <oboInOwl:id>GAZ:00012658</oboInOwl:id>
        <rdfs:label>Chimbu Province</rdfs:label>
    </owl:NamedIndividual>
    


    <!-- http://purl.obolibrary.org/obo/GAZ_00012659 -->

    <owl:NamedIndividual rdf:about="http://purl.obolibrary.org/obo/GAZ_00012659">
        <rdf:type rdf:resource="http://purl.obolibrary.org/obo/ENVO_00000104"/>
        <obo:RO_0001025 rdf:resource="http://purl.obolibrary.org/obo/GAZ_00117921"/>
        <obo:IAO_0000115>A province of Papua New Guinea located on the southern coast. The provincial capital is Kerema. The southern border of the gulf is defined as a line from the southwestern corner of the Fly River Delta in the west, to Cape Suckling 355 km east of this, which is 70 km northwest of Port Moresby.</obo:IAO_0000115>
        <oboInOwl:hasOBONamespace>GAZ</oboInOwl:hasOBONamespace>
        <oboInOwl:id>GAZ:00012659</oboInOwl:id>
        <rdfs:label>Gulf Province</rdfs:label>
    </owl:NamedIndividual>
    


    <!-- http://purl.obolibrary.org/obo/GAZ_00012660 -->

    <owl:NamedIndividual rdf:about="http://purl.obolibrary.org/obo/GAZ_00012660">
        <rdf:type rdf:resource="http://purl.obolibrary.org/obo/ENVO_00000104"/>
        <obo:RO_0001025 rdf:resource="http://purl.obolibrary.org/obo/GAZ_00117918"/>
        <obo:IAO_0000115>A province located in the highlands of Papua New Guinea.</obo:IAO_0000115>
        <oboInOwl:hasOBONamespace>GAZ</oboInOwl:hasOBONamespace>
        <oboInOwl:id>GAZ:00012660</oboInOwl:id>
        <rdfs:label>Enga Province</rdfs:label>
    </owl:NamedIndividual>
    


    <!-- http://purl.obolibrary.org/obo/GAZ_00012661 -->

    <owl:NamedIndividual rdf:about="http://purl.obolibrary.org/obo/GAZ_00012661">
        <rdf:type rdf:resource="http://purl.obolibrary.org/obo/ENVO_00000104"/>
        <obo:RO_0001025 rdf:resource="http://purl.obolibrary.org/obo/GAZ_00117918"/>
        <obo:IAO_0000115>A province of Papua New Guinea. The provincial capital is Mount Hagen.</obo:IAO_0000115>
        <oboInOwl:hasOBONamespace>GAZ</oboInOwl:hasOBONamespace>
        <oboInOwl:id>GAZ:00012661</oboInOwl:id>
        <rdfs:label>Western Highlands Province</rdfs:label>
    </owl:NamedIndividual>
    


    <!-- http://purl.obolibrary.org/obo/GAZ_00012662 -->

    <owl:NamedIndividual rdf:about="http://purl.obolibrary.org/obo/GAZ_00012662">
        <obo:RO_0001025 rdf:resource="http://purl.obolibrary.org/obo/GAZ_00117921"/>
        <obo:IAO_0000115>A coastal province of Papua New Guinea. The provincial capital is Popondetta.</obo:IAO_0000115>
        <oboInOwl:hasOBONamespace>GAZ</oboInOwl:hasOBONamespace>
        <oboInOwl:id>GAZ:00012662</oboInOwl:id>
        <rdfs:label>Northern Province</rdfs:label>
    </owl:NamedIndividual>
    


    <!-- http://purl.obolibrary.org/obo/GAZ_00012663 -->

    <owl:NamedIndividual rdf:about="http://purl.obolibrary.org/obo/GAZ_00012663">
        <obo:RO_0001025 rdf:resource="http://purl.obolibrary.org/obo/GAZ_00117919"/>
        <obo:IAO_0000115>The north-westernmost province of Papua New Guinea.</obo:IAO_0000115>
        <oboInOwl:hasOBONamespace>GAZ</oboInOwl:hasOBONamespace>
        <oboInOwl:id>GAZ:00012663</oboInOwl:id>
        <rdfs:label>Sandaun Province</rdfs:label>
    </owl:NamedIndividual>
    


    <!-- http://purl.obolibrary.org/obo/GAZ_00012664 -->

    <owl:NamedIndividual rdf:about="http://purl.obolibrary.org/obo/GAZ_00012664">
        <rdf:type rdf:resource="http://purl.obolibrary.org/obo/ENVO_00000104"/>
        <obo:RO_0001025 rdf:resource="http://purl.obolibrary.org/obo/GAZ_00117918"/>
        <obo:IAO_0000115>A province in Papua New Guinea. Its provincial capital is the town of Mendi.</obo:IAO_0000115>
        <oboInOwl:hasOBONamespace>GAZ</oboInOwl:hasOBONamespace>
        <oboInOwl:id>GAZ:00012664</oboInOwl:id>
        <rdfs:label>Southern Highlands Province</rdfs:label>
    </owl:NamedIndividual>
    


    <!-- http://purl.obolibrary.org/obo/GAZ_00012665 -->

    <owl:NamedIndividual rdf:about="http://purl.obolibrary.org/obo/GAZ_00012665">
        <obo:RO_0001025 rdf:resource="http://purl.obolibrary.org/obo/GAZ_00117921"/>
        <obo:IAO_0000115>A coastal province in southwestern Papua New Guinea, bordering the Indonesian province of Papua. The provincial capital is Daru, on the island of Daru.</obo:IAO_0000115>
        <oboInOwl:hasOBONamespace>GAZ</oboInOwl:hasOBONamespace>
        <oboInOwl:id>GAZ:00012665</oboInOwl:id>
        <rdfs:label>Western Province</rdfs:label>
    </owl:NamedIndividual>
    


    <!-- http://purl.obolibrary.org/obo/GAZ_00012666 -->

    <owl:NamedIndividual rdf:about="http://purl.obolibrary.org/obo/GAZ_00012666">
        <rdf:type rdf:resource="http://purl.obolibrary.org/obo/ENVO_00000104"/>
        <obo:RO_0001025 rdf:resource="http://purl.obolibrary.org/obo/GAZ_00117921"/>
        <obo:IAO_0000115>A province of Papua New Guinea. Its capital is Alotau.</obo:IAO_0000115>
        <oboInOwl:hasOBONamespace>GAZ</oboInOwl:hasOBONamespace>
        <oboInOwl:id>GAZ:00012666</oboInOwl:id>
        <rdfs:label>Milne Bay Province</rdfs:label>
    </owl:NamedIndividual>
    


    <!-- http://purl.obolibrary.org/obo/GAZ_00012667 -->

    <owl:NamedIndividual rdf:about="http://purl.obolibrary.org/obo/GAZ_00012667">
        <obo:RO_0001025 rdf:resource="http://purl.obolibrary.org/obo/GAZ_00117920"/>
        <obo:IAO_0000115>The smallest province in Papua New Guinea. The province is made up of the Admiralty Islands (a group of 18 islands in the Bismarck Archipelago) and Wuvulu Island and nearby atolls in the west. The largest island in the group is Manus Island where Lorengau is located.</obo:IAO_0000115>
        <oboInOwl:hasOBONamespace>GAZ</oboInOwl:hasOBONamespace>
        <oboInOwl:id>GAZ:00012667</oboInOwl:id>
        <rdfs:label>Manus Province</rdfs:label>
    </owl:NamedIndividual>
    


    <!-- http://purl.obolibrary.org/obo/GAZ_00016805 -->

    <owl:NamedIndividual rdf:about="http://purl.obolibrary.org/obo/GAZ_00016805">
        <obo:RO_0001025 rdf:resource="http://purl.obolibrary.org/obo/GAZ_00005192"/>
        <obo:RO_0001025 rdf:resource="http://purl.obolibrary.org/obo/GAZ_00005193"/>
        <obo:IAO_0000115>A group of islands located in East New Britain Province, Papua New Guinea. They are found in St George&apos;s Channel between New Britain and New Ireland islands and form part of Bismarck Archipelago.</obo:IAO_0000115>
        <oboInOwl:hasOBONamespace>GAZ</oboInOwl:hasOBONamespace>
        <oboInOwl:id>GAZ:00016805</oboInOwl:id>
        <rdfs:label>Duke of York Islands</rdfs:label>
    </owl:NamedIndividual>
    


    <!-- http://purl.obolibrary.org/obo/GAZ_00016806 -->

    <owl:NamedIndividual rdf:about="http://purl.obolibrary.org/obo/GAZ_00016806">
        <obo:RO_0001025 rdf:resource="http://purl.obolibrary.org/obo/GAZ_00016805"/>
        <obo:IAO_0000115>One of the Duke of York Islands.</obo:IAO_0000115>
        <oboInOwl:hasOBONamespace>GAZ</oboInOwl:hasOBONamespace>
        <oboInOwl:id>GAZ:00016806</oboInOwl:id>
        <rdfs:label>Kabakon Island</rdfs:label>
    </owl:NamedIndividual>
    


    <!-- http://purl.obolibrary.org/obo/GAZ_00016807 -->

    <owl:NamedIndividual rdf:about="http://purl.obolibrary.org/obo/GAZ_00016807">
        <obo:RO_0001025 rdf:resource="http://purl.obolibrary.org/obo/GAZ_00016805"/>
        <obo:IAO_0000115>One of the Duke of York Islands.</obo:IAO_0000115>
        <oboInOwl:hasOBONamespace>GAZ</oboInOwl:hasOBONamespace>
        <oboInOwl:id>GAZ:00016807</oboInOwl:id>
        <rdfs:label>Ulu Island</rdfs:label>
    </owl:NamedIndividual>
    


    <!-- http://purl.obolibrary.org/obo/GAZ_00016808 -->

    <owl:NamedIndividual rdf:about="http://purl.obolibrary.org/obo/GAZ_00016808">
        <obo:RO_0001025 rdf:resource="http://purl.obolibrary.org/obo/GAZ_00016805"/>
        <obo:IAO_0000115>One of the Duke of York Islands.</obo:IAO_0000115>
        <oboInOwl:hasOBONamespace>GAZ</oboInOwl:hasOBONamespace>
        <oboInOwl:id>GAZ:00016808</oboInOwl:id>
        <rdfs:label>Mioko Island</rdfs:label>
    </owl:NamedIndividual>
    


    <!-- http://purl.obolibrary.org/obo/GAZ_00016809 -->

    <owl:NamedIndividual rdf:about="http://purl.obolibrary.org/obo/GAZ_00016809">
        <obo:RO_0001025 rdf:resource="http://purl.obolibrary.org/obo/GAZ_00016805"/>
        <obo:IAO_0000115>One of the Duke of York Islands.</obo:IAO_0000115>
        <oboInOwl:hasOBONamespace>GAZ</oboInOwl:hasOBONamespace>
        <oboInOwl:id>GAZ:00016809</oboInOwl:id>
        <rdfs:label>Kerawara Island</rdfs:label>
    </owl:NamedIndividual>
    


    <!-- http://purl.obolibrary.org/obo/GAZ_00016810 -->

    <owl:NamedIndividual rdf:about="http://purl.obolibrary.org/obo/GAZ_00016810">
        <obo:RO_0001025 rdf:resource="http://purl.obolibrary.org/obo/GAZ_00016805"/>
        <obo:IAO_0000115>One of the Duke of York Islands.</obo:IAO_0000115>
        <oboInOwl:hasOBONamespace>GAZ</oboInOwl:hasOBONamespace>
        <oboInOwl:id>GAZ:00016810</oboInOwl:id>
        <rdfs:label>Makada Island</rdfs:label>
    </owl:NamedIndividual>
    


    <!-- http://purl.obolibrary.org/obo/GAZ_00016811 -->

    <owl:NamedIndividual rdf:about="http://purl.obolibrary.org/obo/GAZ_00016811">
        <obo:RO_0001025 rdf:resource="http://purl.obolibrary.org/obo/GAZ_00016805"/>
        <obo:IAO_0000115>The largest island of Duke of York Islands, Papua New Guinea.</obo:IAO_0000115>
        <oboInOwl:hasOBONamespace>GAZ</oboInOwl:hasOBONamespace>
        <oboInOwl:id>GAZ:00016811</oboInOwl:id>
        <rdfs:label>Duke of York Island</rdfs:label>
    </owl:NamedIndividual>
    


    <!-- http://purl.obolibrary.org/obo/GAZ_00016812 -->

    <owl:NamedIndividual rdf:about="http://purl.obolibrary.org/obo/GAZ_00016812">
        <rdf:type rdf:resource="http://purl.obolibrary.org/obo/ENVO_00000130"/>
        <obo:RO_0001025 rdf:resource="http://purl.obolibrary.org/obo/GAZ_00007179"/>
        <obo:IAO_0000115>A small group of volcanic islands and reefs of the Saint Andrew Strait region of the Admiralty Islands. The islands are located 5.5 km southeast from Lou and 5 km northeast from the Pam Islands.</obo:IAO_0000115>
        <oboInOwl:hasOBONamespace>GAZ</oboInOwl:hasOBONamespace>
        <oboInOwl:id>GAZ:00016812</oboInOwl:id>
        <rdfs:label>Saint Andrews Islands</rdfs:label>
    </owl:NamedIndividual>
    


    <!-- http://purl.obolibrary.org/obo/GAZ_00016813 -->

    <owl:NamedIndividual rdf:about="http://purl.obolibrary.org/obo/GAZ_00016813">
        <obo:RO_0001025 rdf:resource="http://purl.obolibrary.org/obo/GAZ_00007179"/>
        <obo:IAO_0000115>One of the Admiralty Islands in the Bismarck Archipelago.</obo:IAO_0000115>
        <oboInOwl:hasOBONamespace>GAZ</oboInOwl:hasOBONamespace>
        <oboInOwl:id>GAZ:00016813</oboInOwl:id>
        <rdfs:label>Rambutyo Island</rdfs:label>
    </owl:NamedIndividual>
    


    <!-- http://purl.obolibrary.org/obo/GAZ_00016814 -->

    <owl:NamedIndividual rdf:about="http://purl.obolibrary.org/obo/GAZ_00016814">
        <obo:RO_0001025 rdf:resource="http://purl.obolibrary.org/obo/GAZ_00007179"/>
        <obo:IAO_0000115>An island formed by a Pleistocene stratovolcano with a large summit crater and several flank vents. Some of these might be of Holocene age. In contrast to its neighboring islands to the north, Baluan has erupted basaltic rather than rhyolitic rocks. Sabroma, the elliptical summit crater, has a maximum width of about 1 km. The arcuate rim of the Batapona Mountain pyroclastic cone is prominent at the north edge of the island. Several small islands consisting of cone remnants are located within a km of the north coast. Warm springs occur along the coast.</obo:IAO_0000115>
        <oboInOwl:hasOBONamespace>GAZ</oboInOwl:hasOBONamespace>
        <oboInOwl:id>GAZ:00016814</oboInOwl:id>
        <rdfs:label>Baluan Island</rdfs:label>
    </owl:NamedIndividual>
    


    <!-- http://purl.obolibrary.org/obo/GAZ_00016815 -->

    <owl:NamedIndividual rdf:about="http://purl.obolibrary.org/obo/GAZ_00016815">
        <obo:RO_0001025 rdf:resource="http://purl.obolibrary.org/obo/GAZ_00007179"/>
        <oboInOwl:hasOBONamespace>GAZ</oboInOwl:hasOBONamespace>
        <oboInOwl:id>GAZ:00016815</oboInOwl:id>
        <rdfs:label>Ndrova Island</rdfs:label>
    </owl:NamedIndividual>
    


    <!-- http://purl.obolibrary.org/obo/GAZ_00016816 -->

    <owl:NamedIndividual rdf:about="http://purl.obolibrary.org/obo/GAZ_00016816">
        <obo:RO_0001025 rdf:resource="http://purl.obolibrary.org/obo/GAZ_00007179"/>
        <obo:IAO_0000115>One of the Admiralty Islands.</obo:IAO_0000115>
        <oboInOwl:hasOBONamespace>GAZ</oboInOwl:hasOBONamespace>
        <oboInOwl:id>GAZ:00016816</oboInOwl:id>
        <rdfs:label>Pak Island</rdfs:label>
    </owl:NamedIndividual>
    


    <!-- http://purl.obolibrary.org/obo/GAZ_00016817 -->

    <owl:NamedIndividual rdf:about="http://purl.obolibrary.org/obo/GAZ_00016817">
        <obo:RO_0001025 rdf:resource="http://purl.obolibrary.org/obo/GAZ_00007179"/>
        <obo:IAO_0000115>One of the Admiralty Islands.</obo:IAO_0000115>
        <oboInOwl:hasOBONamespace>GAZ</oboInOwl:hasOBONamespace>
        <oboInOwl:id>GAZ:00016817</oboInOwl:id>
        <rdfs:label>Lou Island</rdfs:label>
    </owl:NamedIndividual>
    


    <!-- http://purl.obolibrary.org/obo/GAZ_00016818 -->

    <owl:NamedIndividual rdf:about="http://purl.obolibrary.org/obo/GAZ_00016818">
        <obo:RO_0001025 rdf:resource="http://purl.obolibrary.org/obo/GAZ_00007179"/>
        <obo:IAO_0000115>The third largest of the Admiralty Islands. It is significant because it contains the main airport of Manus Province on its eastern coastline, at Momote. It is connected to Lorengau, the capital of the province, on Manus Island via a highway and bridge.</obo:IAO_0000115>
        <oboInOwl:hasOBONamespace>GAZ</oboInOwl:hasOBONamespace>
        <oboInOwl:id>GAZ:00016818</oboInOwl:id>
        <rdfs:label>Los Negros Island</rdfs:label>
    </owl:NamedIndividual>
    


    <!-- http://purl.obolibrary.org/obo/GAZ_00016819 -->

    <owl:NamedIndividual rdf:about="http://purl.obolibrary.org/obo/GAZ_00016819">
        <rdf:type rdf:resource="http://purl.obolibrary.org/obo/ENVO_00000222"/>
        <obo:RO_0001025 rdf:resource="http://purl.obolibrary.org/obo/GAZ_00007179"/>
    </owl:NamedIndividual>
    


    <!-- http://purl.obolibrary.org/obo/GAZ_00016820 -->

    <owl:NamedIndividual rdf:about="http://purl.obolibrary.org/obo/GAZ_00016820">
        <obo:RO_0001025 rdf:resource="http://purl.obolibrary.org/obo/GAZ_00007179"/>
        <obo:IAO_0000115>One of the Admiralty Islands.</obo:IAO_0000115>
        <oboInOwl:hasOBONamespace>GAZ</oboInOwl:hasOBONamespace>
        <oboInOwl:id>GAZ:00016820</oboInOwl:id>
        <rdfs:label>Tong Island</rdfs:label>
    </owl:NamedIndividual>
    


    <!-- http://purl.obolibrary.org/obo/GAZ_00016821 -->

    <owl:NamedIndividual rdf:about="http://purl.obolibrary.org/obo/GAZ_00016821">
        <rdf:type rdf:resource="http://purl.obolibrary.org/obo/ENVO_00000130"/>
        <obo:RO_0001025 rdf:resource="http://purl.obolibrary.org/obo/GAZ_00005193"/>
        <obo:IAO_0000115>A loose collection of small islets and reefs located at the southern edge of the Admiralty Islands; the nearest neighbours to the Purdy Island are Manus, 69 km to the north, and the Alim Islands, 60 km to the west.</obo:IAO_0000115>
        <oboInOwl:hasOBONamespace>GAZ</oboInOwl:hasOBONamespace>
        <oboInOwl:id>GAZ:00016821</oboInOwl:id>
        <rdfs:label>Purdy Islands</rdfs:label>
    </owl:NamedIndividual>
    


    <!-- http://purl.obolibrary.org/obo/GAZ_00016822 -->

    <owl:NamedIndividual rdf:about="http://purl.obolibrary.org/obo/GAZ_00016822">
        <obo:RO_0001025 rdf:resource="http://purl.obolibrary.org/obo/GAZ_00005193"/>
        <obo:IAO_0000115>A group of islands in the Bismarck Archipelago, part of Papua New Guinea, off the NE coast of New Guinea in the western Pacific Ocean.</obo:IAO_0000115>
        <oboInOwl:hasOBONamespace>GAZ</oboInOwl:hasOBONamespace>
        <oboInOwl:id>GAZ:00016822</oboInOwl:id>
        <rdfs:label>Western Islands</rdfs:label>
    </owl:NamedIndividual>
    


    <!-- http://purl.obolibrary.org/obo/GAZ_00016823 -->

    <owl:NamedIndividual rdf:about="http://purl.obolibrary.org/obo/GAZ_00016823">
        <rdf:type rdf:resource="http://purl.obolibrary.org/obo/ENVO_00000222"/>
        <obo:RO_0001025 rdf:resource="http://purl.obolibrary.org/obo/GAZ_00022398"/>
        <obo:RO_0001025 rdf:resource="http://purl.obolibrary.org/obo/GAZ_00118102"/>
        <obo:IAO_0000115>A large volcanic island in New Ireland Province, part of the Bismarck Archipelago of the New Guinea Islands region of Papua New Guinea.</obo:IAO_0000115>
        <oboInOwl:hasOBONamespace>GAZ</oboInOwl:hasOBONamespace>
        <oboInOwl:id>GAZ:00016823</oboInOwl:id>
        <rdfs:label>New Hanover Island</rdfs:label>
    </owl:NamedIndividual>
    


    <!-- http://purl.obolibrary.org/obo/GAZ_00016824 -->

    <owl:NamedIndividual rdf:about="http://purl.obolibrary.org/obo/GAZ_00016824">
        <rdf:type rdf:resource="http://purl.obolibrary.org/obo/ENVO_00000220"/>
        <obo:RO_0001025 rdf:resource="http://purl.obolibrary.org/obo/GAZ_00022398"/>
        <obo:RO_0001025 rdf:resource="http://purl.obolibrary.org/obo/GAZ_00118107"/>
        <obo:IAO_0000115>An island group in Papua New Guinea, located east of New Ireland.</obo:IAO_0000115>
        <oboInOwl:hasOBONamespace>GAZ</oboInOwl:hasOBONamespace>
        <oboInOwl:id>GAZ:00016824</oboInOwl:id>
        <rdfs:label>Feni Islands</rdfs:label>
    </owl:NamedIndividual>
    


    <!-- http://purl.obolibrary.org/obo/GAZ_00016825 -->

    <owl:NamedIndividual rdf:about="http://purl.obolibrary.org/obo/GAZ_00016825">
        <obo:RO_0001025 rdf:resource="http://purl.obolibrary.org/obo/GAZ_00016824"/>
        <obo:IAO_0000115>A stratovolcanic island which, together with Babase, another volcanic island, is one of the two Feni Islands in the Bismarck Archipelago. The island is located within the Papua New Guinea&apos;s New Ireland Province, to the east of the island of New Ireland. A dominantly Pliocene-to-Pleistocene stratovolcano characterized by a variety of alkalic rocks types. A 3 km wide central caldera was constructed over Tertiary marine limestone deposits and is occupied by late-Pleistocene trachytic lava domes. A maar on the eastern side of the domes formed about 2300 years ago. Several thermal areas, consisting of hot and boiling springs, mud pools, and low-temperature fumaroles, are found on the western side of the caldera floor and near the western edge of the central lava dome. Shallow-water hydrothermal venting also occurs in a coral reef environment just off the western coast of the island. Babase Island, immediately to the NE of Ambitle, is composed of a Pleistocene stratovolcano and lava dome connected by a narrow isthmus.</obo:IAO_0000115>
        <oboInOwl:hasOBONamespace>GAZ</oboInOwl:hasOBONamespace>
        <oboInOwl:id>GAZ:00016825</oboInOwl:id>
        <rdfs:label>Ambitle Island</rdfs:label>
    </owl:NamedIndividual>
    


    <!-- http://purl.obolibrary.org/obo/GAZ_00016826 -->

    <owl:NamedIndividual rdf:about="http://purl.obolibrary.org/obo/GAZ_00016826">
        <obo:RO_0001025 rdf:resource="http://purl.obolibrary.org/obo/GAZ_00016824"/>
        <obo:IAO_0000115>An island of the Feni Islands in Papua New Guinea, located east of New Ireland. It consists of a stratovolcano and a lava dome, joined by an isthmus.</obo:IAO_0000115>
        <oboInOwl:hasOBONamespace>GAZ</oboInOwl:hasOBONamespace>
        <oboInOwl:id>GAZ:00016826</oboInOwl:id>
        <rdfs:label>Babase Island</rdfs:label>
    </owl:NamedIndividual>
    


    <!-- http://purl.obolibrary.org/obo/GAZ_00016827 -->

    <owl:NamedIndividual rdf:about="http://purl.obolibrary.org/obo/GAZ_00016827">
        <rdf:type rdf:resource="http://purl.obolibrary.org/obo/ENVO_00000220"/>
        <obo:RO_0001025 rdf:resource="http://purl.obolibrary.org/obo/GAZ_00022398"/>
        <obo:RO_0001025 rdf:resource="http://purl.obolibrary.org/obo/GAZ_00118106"/>
        <obo:IAO_0000115>An island group in Papua New Guinea, located north of New Ireland.</obo:IAO_0000115>
        <oboInOwl:hasOBONamespace>GAZ</oboInOwl:hasOBONamespace>
        <oboInOwl:id>GAZ:00016827</oboInOwl:id>
        <rdfs:label>Lihir Islands</rdfs:label>
    </owl:NamedIndividual>
    


    <!-- http://purl.obolibrary.org/obo/GAZ_00016828 -->

    <owl:NamedIndividual rdf:about="http://purl.obolibrary.org/obo/GAZ_00016828">
        <obo:RO_0001025 rdf:resource="http://purl.obolibrary.org/obo/GAZ_00016827"/>
        <oboInOwl:hasOBONamespace>GAZ</oboInOwl:hasOBONamespace>
        <oboInOwl:id>GAZ:00016828</oboInOwl:id>
        <rdfs:label>Mahur Island</rdfs:label>
    </owl:NamedIndividual>
    


    <!-- http://purl.obolibrary.org/obo/GAZ_00016829 -->

    <owl:NamedIndividual rdf:about="http://purl.obolibrary.org/obo/GAZ_00016829">
        <obo:RO_0001025 rdf:resource="http://purl.obolibrary.org/obo/GAZ_00016827"/>
        <oboInOwl:hasOBONamespace>GAZ</oboInOwl:hasOBONamespace>
        <oboInOwl:id>GAZ:00016829</oboInOwl:id>
        <rdfs:label>Mali Island</rdfs:label>
    </owl:NamedIndividual>
    


    <!-- http://purl.obolibrary.org/obo/GAZ_00016830 -->

    <owl:NamedIndividual rdf:about="http://purl.obolibrary.org/obo/GAZ_00016830">
        <obo:RO_0001025 rdf:resource="http://purl.obolibrary.org/obo/GAZ_00016827"/>
        <oboInOwl:hasOBONamespace>GAZ</oboInOwl:hasOBONamespace>
        <oboInOwl:id>GAZ:00016830</oboInOwl:id>
        <rdfs:label>Sanambiet Island</rdfs:label>
    </owl:NamedIndividual>
    


    <!-- http://purl.obolibrary.org/obo/GAZ_00016831 -->

    <owl:NamedIndividual rdf:about="http://purl.obolibrary.org/obo/GAZ_00016831">
        <obo:RO_0001025 rdf:resource="http://purl.obolibrary.org/obo/GAZ_00016827"/>
        <obo:IAO_0000115>An island composed of a Pliocene-to-Holocene volcanic complex of several overlapping basaltic stratovolcanoes. The youngest volcano, Luise, contains an elliptical, 5.5 km wide caldera that is breached by the sea on the NE side as a result of edifice collapse about 0.4 million years ago, forming Luise Harbor. The flanks of the volcano are only moderately dissected. The steep-sided caldera wall rises to 700 m above sea level. A central lava plug is strongly hydrothermally altered and displays extensive thermal activity along its margins. Thermal activity includes boiling hot springs, mud pools, and sulfur-encrusted low-temperature fumaroles. The Ladolam hydrothermal deposit hosts one of the youngest and largest gold deposits in the world, which is now being extracted by open-pit mining. The near-surface, epithermal gold deposition extends to about 400 m below sea level over an area of about 2 sq km.</obo:IAO_0000115>
        <oboInOwl:hasOBONamespace>GAZ</oboInOwl:hasOBONamespace>
        <oboInOwl:id>GAZ:00016831</oboInOwl:id>
        <rdfs:label>Lihir Island</rdfs:label>
    </owl:NamedIndividual>
    


    <!-- http://purl.obolibrary.org/obo/GAZ_00016832 -->

    <owl:NamedIndividual rdf:about="http://purl.obolibrary.org/obo/GAZ_00016832">
        <obo:RO_0001025 rdf:resource="http://purl.obolibrary.org/obo/GAZ_00016827"/>
        <oboInOwl:hasOBONamespace>GAZ</oboInOwl:hasOBONamespace>
        <oboInOwl:id>GAZ:00016832</oboInOwl:id>
        <rdfs:label>Masahet Island</rdfs:label>
    </owl:NamedIndividual>
    


    <!-- http://purl.obolibrary.org/obo/GAZ_00016833 -->

    <owl:NamedIndividual rdf:about="http://purl.obolibrary.org/obo/GAZ_00016833">
        <rdf:type rdf:resource="http://purl.obolibrary.org/obo/ENVO_00000220"/>
        <obo:RO_0001025 rdf:resource="http://purl.obolibrary.org/obo/GAZ_00022398"/>
        <obo:RO_0001025 rdf:resource="http://purl.obolibrary.org/obo/GAZ_00118109"/>
        <obo:IAO_0000115>An island group in Papua New Guinea, located north of New Ireland. It is a part of the Bismarck Archipelago. The group contains Tabar Island, Tatau Island and Simberi Island.</obo:IAO_0000115>
        <oboInOwl:hasOBONamespace>GAZ</oboInOwl:hasOBONamespace>
        <oboInOwl:id>GAZ:00016833</oboInOwl:id>
        <rdfs:label>Tabar Islands</rdfs:label>
    </owl:NamedIndividual>
    


    <!-- http://purl.obolibrary.org/obo/GAZ_00016834 -->

    <owl:NamedIndividual rdf:about="http://purl.obolibrary.org/obo/GAZ_00016834">
        <rdf:type rdf:resource="http://purl.obolibrary.org/obo/ENVO_00000222"/>
        <obo:RO_0001025 rdf:resource="http://purl.obolibrary.org/obo/GAZ_00016833"/>
        <obo:IAO_0000115>A volcanic island in the Tabar Group in Papua New Guinea&apos;s New Ireland Province.</obo:IAO_0000115>
        <oboInOwl:hasOBONamespace>GAZ</oboInOwl:hasOBONamespace>
        <oboInOwl:id>GAZ:00016834</oboInOwl:id>
        <rdfs:label>Simberi Island</rdfs:label>
    </owl:NamedIndividual>
    


    <!-- http://purl.obolibrary.org/obo/GAZ_00016835 -->

    <owl:NamedIndividual rdf:about="http://purl.obolibrary.org/obo/GAZ_00016835">
        <obo:RO_0001025 rdf:resource="http://purl.obolibrary.org/obo/GAZ_00016833"/>
        <obo:IAO_0000115>One of the Tabar Islands.</obo:IAO_0000115>
        <oboInOwl:hasOBONamespace>GAZ</oboInOwl:hasOBONamespace>
        <oboInOwl:id>GAZ:00016835</oboInOwl:id>
        <rdfs:label>Tabar Island</rdfs:label>
    </owl:NamedIndividual>
    


    <!-- http://purl.obolibrary.org/obo/GAZ_00016836 -->

    <owl:NamedIndividual rdf:about="http://purl.obolibrary.org/obo/GAZ_00016836">
        <obo:RO_0001025 rdf:resource="http://purl.obolibrary.org/obo/GAZ_00016833"/>
        <obo:IAO_0000115>One of the Tabar Islands.</obo:IAO_0000115>
        <oboInOwl:hasOBONamespace>GAZ</oboInOwl:hasOBONamespace>
        <oboInOwl:id>GAZ:00016836</oboInOwl:id>
        <rdfs:label>Tatau Island</rdfs:label>
    </owl:NamedIndividual>
    


    <!-- http://purl.obolibrary.org/obo/GAZ_00016837 -->

    <owl:NamedIndividual rdf:about="http://purl.obolibrary.org/obo/GAZ_00016837">
        <rdf:type rdf:resource="http://purl.obolibrary.org/obo/ENVO_00000220"/>
        <obo:RO_0001025 rdf:resource="http://purl.obolibrary.org/obo/GAZ_00022398"/>
        <obo:RO_0001025 rdf:resource="http://purl.obolibrary.org/obo/GAZ_00118107"/>
        <obo:IAO_0000115>An island group in Papua New Guinea, located northeast of New Ireland and part of the Bismarck Archipelago. The islands are the remnants of a stratovolcano which collapsed to form a caldera.</obo:IAO_0000115>
        <oboInOwl:hasOBONamespace>GAZ</oboInOwl:hasOBONamespace>
        <oboInOwl:id>GAZ:00016837</oboInOwl:id>
        <rdfs:label>Tanga Islands</rdfs:label>
    </owl:NamedIndividual>
    


    <!-- http://purl.obolibrary.org/obo/GAZ_00016838 -->

    <owl:NamedIndividual rdf:about="http://purl.obolibrary.org/obo/GAZ_00016838">
        <obo:RO_0001025 rdf:resource="http://purl.obolibrary.org/obo/GAZ_00016837"/>
        <obo:IAO_0000115>An island formed from a post-caldera lava dome.</obo:IAO_0000115>
        <oboInOwl:hasOBONamespace>GAZ</oboInOwl:hasOBONamespace>
        <oboInOwl:id>GAZ:00016838</oboInOwl:id>
        <rdfs:label>Bitlik Island</rdfs:label>
    </owl:NamedIndividual>
    


    <!-- http://purl.obolibrary.org/obo/GAZ_00016839 -->

    <owl:NamedIndividual rdf:about="http://purl.obolibrary.org/obo/GAZ_00016839">
        <obo:RO_0001025 rdf:resource="http://purl.obolibrary.org/obo/GAZ_00016837"/>
        <obo:IAO_0000115>An island formed from a post-caldera lava dome.</obo:IAO_0000115>
        <oboInOwl:hasOBONamespace>GAZ</oboInOwl:hasOBONamespace>
        <oboInOwl:id>GAZ:00016839</oboInOwl:id>
        <rdfs:label>Bitbok Island</rdfs:label>
    </owl:NamedIndividual>
    


    <!-- http://purl.obolibrary.org/obo/GAZ_00016840 -->

    <owl:NamedIndividual rdf:about="http://purl.obolibrary.org/obo/GAZ_00016840">
        <obo:RO_0001025 rdf:resource="http://purl.obolibrary.org/obo/GAZ_00016837"/>
        <obo:IAO_0000115>An island on the Tanga Caldera rim.</obo:IAO_0000115>
        <oboInOwl:hasOBONamespace>GAZ</oboInOwl:hasOBONamespace>
        <oboInOwl:id>GAZ:00016840</oboInOwl:id>
        <rdfs:label>Lif Island</rdfs:label>
    </owl:NamedIndividual>
    


    <!-- http://purl.obolibrary.org/obo/GAZ_00016841 -->

    <owl:NamedIndividual rdf:about="http://purl.obolibrary.org/obo/GAZ_00016841">
        <obo:RO_0001025 rdf:resource="http://purl.obolibrary.org/obo/GAZ_00016837"/>
        <obo:IAO_0000115>An island on the Tanga Caldera rim.</obo:IAO_0000115>
        <oboInOwl:hasOBONamespace>GAZ</oboInOwl:hasOBONamespace>
        <oboInOwl:id>GAZ:00016841</oboInOwl:id>
        <rdfs:label>Malendok Island</rdfs:label>
    </owl:NamedIndividual>
    


    <!-- http://purl.obolibrary.org/obo/GAZ_00016842 -->

    <owl:NamedIndividual rdf:about="http://purl.obolibrary.org/obo/GAZ_00016842">
        <obo:RO_0001025 rdf:resource="http://purl.obolibrary.org/obo/GAZ_00016837"/>
        <obo:IAO_0000115>An island on the Tanga Caldera rim.</obo:IAO_0000115>
        <oboInOwl:hasOBONamespace>GAZ</oboInOwl:hasOBONamespace>
        <oboInOwl:id>GAZ:00016842</oboInOwl:id>
        <rdfs:label>Tefa Island</rdfs:label>
    </owl:NamedIndividual>
    


    <!-- http://purl.obolibrary.org/obo/GAZ_00016843 -->

    <owl:NamedIndividual rdf:about="http://purl.obolibrary.org/obo/GAZ_00016843">
        <obo:RO_0001025 rdf:resource="http://purl.obolibrary.org/obo/GAZ_00007180"/>
        <obo:IAO_0000115>One of the Saint Matthias Islands.</obo:IAO_0000115>
        <oboInOwl:hasOBONamespace>GAZ</oboInOwl:hasOBONamespace>
        <oboInOwl:id>GAZ:00016843</oboInOwl:id>
        <rdfs:label>Emirau Island</rdfs:label>
    </owl:NamedIndividual>
    


    <!-- http://purl.obolibrary.org/obo/GAZ_00016844 -->

    <owl:NamedIndividual rdf:about="http://purl.obolibrary.org/obo/GAZ_00016844">
        <obo:RO_0001025 rdf:resource="http://purl.obolibrary.org/obo/GAZ_00007180"/>
        <obo:IAO_0000115>One of the Saint Matthias Islands.</obo:IAO_0000115>
        <oboInOwl:hasOBONamespace>GAZ</oboInOwl:hasOBONamespace>
        <oboInOwl:id>GAZ:00016844</oboInOwl:id>
        <rdfs:label>Eloaua Island</rdfs:label>
    </owl:NamedIndividual>
    


    <!-- http://purl.obolibrary.org/obo/GAZ_00016845 -->

    <owl:NamedIndividual rdf:about="http://purl.obolibrary.org/obo/GAZ_00016845">
        <obo:RO_0001025 rdf:resource="http://purl.obolibrary.org/obo/GAZ_00007180"/>
        <obo:IAO_0000115>One of the Saint Matthias Islands.</obo:IAO_0000115>
        <oboInOwl:hasOBONamespace>GAZ</oboInOwl:hasOBONamespace>
        <oboInOwl:id>GAZ:00016845</oboInOwl:id>
        <rdfs:label>Mussau Island</rdfs:label>
    </owl:NamedIndividual>
    


    <!-- http://purl.obolibrary.org/obo/GAZ_00016846 -->

    <owl:NamedIndividual rdf:about="http://purl.obolibrary.org/obo/GAZ_00016846">
        <obo:RO_0001025 rdf:resource="http://purl.obolibrary.org/obo/GAZ_00016847"/>
        <obo:IAO_0000115>A low, 12 km wide elongated island that is cut by a 5 km wide caldera that is flooded by the sea through a narrow breach on the southern side of the island, forming Johann Albrecht harbor. The steep-sided caldera walls rise 100-150 m above the sea. Satellitic cones were constructed along the NE and SW coasts.</obo:IAO_0000115>
        <oboInOwl:hasOBONamespace>GAZ</oboInOwl:hasOBONamespace>
        <oboInOwl:id>GAZ:00016846</oboInOwl:id>
        <rdfs:label>Garove Island</rdfs:label>
    </owl:NamedIndividual>
    


    <!-- http://purl.obolibrary.org/obo/GAZ_00016847 -->

    <owl:NamedIndividual rdf:about="http://purl.obolibrary.org/obo/GAZ_00016847">
        <obo:RO_0001025 rdf:resource="http://purl.obolibrary.org/obo/GAZ_00005193"/>
        <obo:IAO_0000115>A volcanic island group with an area of 96 km2 located in the Bismarck Archipelago volcanic island group, a part of Papua New Guinea in the South West Pacific, which has a total area of 49,730 km2.</obo:IAO_0000115>
        <oboInOwl:hasOBONamespace>GAZ</oboInOwl:hasOBONamespace>
        <oboInOwl:id>GAZ:00016847</oboInOwl:id>
        <rdfs:label>Vitu Islands</rdfs:label>
    </owl:NamedIndividual>
    


    <!-- http://purl.obolibrary.org/obo/GAZ_00016848 -->

    <owl:NamedIndividual rdf:about="http://purl.obolibrary.org/obo/GAZ_00016848">
        <obo:RO_0001025 rdf:resource="http://purl.obolibrary.org/obo/GAZ_00016847"/>
        <obo:IAO_0000115>One of the Vitu Islands.</obo:IAO_0000115>
        <oboInOwl:hasOBONamespace>GAZ</oboInOwl:hasOBONamespace>
        <oboInOwl:id>GAZ:00016848</oboInOwl:id>
        <rdfs:label>Unea Island</rdfs:label>
    </owl:NamedIndividual>
    


    <!-- http://purl.obolibrary.org/obo/GAZ_00016849 -->

    <owl:NamedIndividual rdf:about="http://purl.obolibrary.org/obo/GAZ_00016849">
        <obo:RO_0001025 rdf:resource="http://purl.obolibrary.org/obo/GAZ_00118100"/>
        <obo:IAO_0000115>The second largest island in the Papua New Guinean province of Bougainville.</obo:IAO_0000115>
        <oboInOwl:hasOBONamespace>GAZ</oboInOwl:hasOBONamespace>
        <oboInOwl:id>GAZ:00016849</oboInOwl:id>
        <rdfs:label>Buka Island</rdfs:label>
    </owl:NamedIndividual>
    


    <!-- http://purl.obolibrary.org/obo/GAZ_00016850 -->

    <owl:NamedIndividual rdf:about="http://purl.obolibrary.org/obo/GAZ_00016850">
        <obo:RO_0001025 rdf:resource="http://purl.obolibrary.org/obo/GAZ_00005186"/>
        <obo:IAO_0000115>An island of the Carteret Group.</obo:IAO_0000115>
        <oboInOwl:hasOBONamespace>GAZ</oboInOwl:hasOBONamespace>
        <oboInOwl:id>GAZ:00016850</oboInOwl:id>
        <rdfs:label>Han Island</rdfs:label>
    </owl:NamedIndividual>
    


    <!-- http://purl.obolibrary.org/obo/GAZ_00016851 -->

    <owl:NamedIndividual rdf:about="http://purl.obolibrary.org/obo/GAZ_00016851">
        <obo:RO_0001025 rdf:resource="http://purl.obolibrary.org/obo/GAZ_00005186"/>
        <obo:IAO_0000115>An island of the Carteret Group.</obo:IAO_0000115>
        <oboInOwl:hasOBONamespace>GAZ</oboInOwl:hasOBONamespace>
        <oboInOwl:id>GAZ:00016851</oboInOwl:id>
        <rdfs:label>Yolasa Island</rdfs:label>
    </owl:NamedIndividual>
    


    <!-- http://purl.obolibrary.org/obo/GAZ_00016852 -->

    <owl:NamedIndividual rdf:about="http://purl.obolibrary.org/obo/GAZ_00016852">
        <obo:RO_0001025 rdf:resource="http://purl.obolibrary.org/obo/GAZ_00005186"/>
        <obo:IAO_0000115>An island of the Carteret Group.</obo:IAO_0000115>
        <oboInOwl:hasOBONamespace>GAZ</oboInOwl:hasOBONamespace>
        <oboInOwl:id>GAZ:00016852</oboInOwl:id>
        <rdfs:label>Yesila Island</rdfs:label>
    </owl:NamedIndividual>
    


    <!-- http://purl.obolibrary.org/obo/GAZ_00016853 -->

    <owl:NamedIndividual rdf:about="http://purl.obolibrary.org/obo/GAZ_00016853">
        <obo:RO_0001025 rdf:resource="http://purl.obolibrary.org/obo/GAZ_00005186"/>
        <obo:IAO_0000115>An island of the Carteret Group.</obo:IAO_0000115>
        <oboInOwl:hasOBONamespace>GAZ</oboInOwl:hasOBONamespace>
        <oboInOwl:id>GAZ:00016853</oboInOwl:id>
        <rdfs:label>Jangain Island</rdfs:label>
    </owl:NamedIndividual>
    


    <!-- http://purl.obolibrary.org/obo/GAZ_00016854 -->

    <owl:NamedIndividual rdf:about="http://purl.obolibrary.org/obo/GAZ_00016854">
        <obo:RO_0001025 rdf:resource="http://purl.obolibrary.org/obo/GAZ_00007181"/>
        <obo:RO_0001025 rdf:resource="http://purl.obolibrary.org/obo/GAZ_00022382"/>
        <obo:IAO_0000115>An island in the Milne Bay Province of Papua New Guinea. It lies to the east of the mainland, in the Solomon Sea. It is one of the D&apos;Entrecasteaux Islands, is near the Trobriand Islands and should not be confused with Goodenough&apos;s Island.</obo:IAO_0000115>
        <oboInOwl:hasOBONamespace>GAZ</oboInOwl:hasOBONamespace>
        <oboInOwl:id>GAZ:00016854</oboInOwl:id>
        <rdfs:label>Goodenough Island</rdfs:label>
    </owl:NamedIndividual>
    


    <!-- http://purl.obolibrary.org/obo/GAZ_00016855 -->

    <owl:NamedIndividual rdf:about="http://purl.obolibrary.org/obo/GAZ_00016855">
        <obo:RO_0001025 rdf:resource="http://purl.obolibrary.org/obo/GAZ_00007181"/>
        <obo:RO_0001025 rdf:resource="http://purl.obolibrary.org/obo/GAZ_00022380"/>
        <obo:IAO_0000115>The largest island of the D&apos;Entrecasteaux Islands, in Papua New Guinea.</obo:IAO_0000115>
        <oboInOwl:hasOBONamespace>GAZ</oboInOwl:hasOBONamespace>
        <oboInOwl:id>GAZ:00016855</oboInOwl:id>
        <rdfs:label>Ferguson Island</rdfs:label>
    </owl:NamedIndividual>
    


    <!-- http://purl.obolibrary.org/obo/GAZ_00016856 -->

    <owl:NamedIndividual rdf:about="http://purl.obolibrary.org/obo/GAZ_00016856">
        <obo:RO_0001025 rdf:resource="http://purl.obolibrary.org/obo/GAZ_00007181"/>
        <obo:RO_0001025 rdf:resource="http://purl.obolibrary.org/obo/GAZ_00022380"/>
        <obo:IAO_0000115>A volcanic, 400 square mile, L-shaped island in the south of the D&apos;Entrecasteaux Islands group. It is part of Milne Bay Province, Papua New Guinea.</obo:IAO_0000115>
        <oboInOwl:hasOBONamespace>GAZ</oboInOwl:hasOBONamespace>
        <oboInOwl:id>GAZ:00016856</oboInOwl:id>
        <rdfs:label>Normanby Island</rdfs:label>
    </owl:NamedIndividual>
    


    <!-- http://purl.obolibrary.org/obo/GAZ_00016857 -->

    <owl:NamedIndividual rdf:about="http://purl.obolibrary.org/obo/GAZ_00016857">
        <obo:RO_0001025 rdf:resource="http://purl.obolibrary.org/obo/GAZ_00007181"/>
        <obo:RO_0001025 rdf:resource="http://purl.obolibrary.org/obo/GAZ_00022380"/>
        <obo:IAO_0000115>An island, part of D&apos;Entrecasteaux Islands in Papua New Guinea, located east of Fergusson Island in Milne Bay Province.</obo:IAO_0000115>
        <oboInOwl:hasOBONamespace>GAZ</oboInOwl:hasOBONamespace>
        <oboInOwl:id>GAZ:00016857</oboInOwl:id>
        <rdfs:label>Sanaroa Island</rdfs:label>
    </owl:NamedIndividual>
    


    <!-- http://purl.obolibrary.org/obo/GAZ_00016858 -->

    <owl:NamedIndividual rdf:about="http://purl.obolibrary.org/obo/GAZ_00016858">
        <obo:RO_0001025 rdf:resource="http://purl.obolibrary.org/obo/GAZ_00007181"/>
        <obo:RO_0001025 rdf:resource="http://purl.obolibrary.org/obo/GAZ_00022380"/>
        <obo:IAO_0000115>An island, part of D&apos;Entrecasteaux Islands in Papua New Guinea. It is located south of Fergusson Island and north of Normanby Island.</obo:IAO_0000115>
        <oboInOwl:hasOBONamespace>GAZ</oboInOwl:hasOBONamespace>
        <oboInOwl:id>GAZ:00016858</oboInOwl:id>
        <rdfs:label>Dobu Island</rdfs:label>
    </owl:NamedIndividual>
    


    <!-- http://purl.obolibrary.org/obo/GAZ_00016859 -->

    <owl:NamedIndividual rdf:about="http://purl.obolibrary.org/obo/GAZ_00016859">
        <obo:RO_0001025 rdf:resource="http://purl.obolibrary.org/obo/GAZ_00007182"/>
        <obo:IAO_0000115>An island in the Louisiade Archipelago in Milne Bay Province, Papua New Guinea.</obo:IAO_0000115>
        <oboInOwl:hasOBONamespace>GAZ</oboInOwl:hasOBONamespace>
        <oboInOwl:id>GAZ:00016859</oboInOwl:id>
        <rdfs:label>Sideia Island</rdfs:label>
    </owl:NamedIndividual>
    


    <!-- http://purl.obolibrary.org/obo/GAZ_00016860 -->

    <owl:NamedIndividual rdf:about="http://purl.obolibrary.org/obo/GAZ_00016860">
        <obo:RO_0001025 rdf:resource="http://purl.obolibrary.org/obo/GAZ_00007182"/>
        <obo:IAO_0000115>An island in the Louisiade Archipelago in Milne Bay Province, Papua New Guinea. It is located at the eastern end of the New Guinea mainland.</obo:IAO_0000115>
        <oboInOwl:hasOBONamespace>GAZ</oboInOwl:hasOBONamespace>
        <oboInOwl:id>GAZ:00016860</oboInOwl:id>
        <rdfs:label>Basilaki Island</rdfs:label>
    </owl:NamedIndividual>
    


    <!-- http://purl.obolibrary.org/obo/GAZ_00016861 -->

    <owl:NamedIndividual rdf:about="http://purl.obolibrary.org/obo/GAZ_00016861">
        <rdf:type rdf:resource="http://purl.obolibrary.org/obo/ENVO_00000222"/>
        <obo:RO_0001025 rdf:resource="http://purl.obolibrary.org/obo/GAZ_00007182"/>
        <obo:IAO_0000115>A volcanic island in the northwest of Louisiade Archipelago within (Milne Bay Province of Papua New Guinea).</obo:IAO_0000115>
        <oboInOwl:hasOBONamespace>GAZ</oboInOwl:hasOBONamespace>
        <oboInOwl:id>GAZ:00016861</oboInOwl:id>
        <rdfs:label>Misima Island</rdfs:label>
    </owl:NamedIndividual>
    


    <!-- http://purl.obolibrary.org/obo/GAZ_00016862 -->

    <owl:NamedIndividual rdf:about="http://purl.obolibrary.org/obo/GAZ_00016862">
        <obo:RO_0001025 rdf:resource="http://purl.obolibrary.org/obo/GAZ_00007182"/>
        <obo:IAO_0000115>An island 225 miles south-east of New Guinea. The volcanic and reef fringed island is located in the east of the Louisiade Archipelago.</obo:IAO_0000115>
        <oboInOwl:hasOBONamespace>GAZ</oboInOwl:hasOBONamespace>
        <oboInOwl:id>GAZ:00016862</oboInOwl:id>
        <rdfs:label>Vanatinai Island</rdfs:label>
    </owl:NamedIndividual>
    


    <!-- http://purl.obolibrary.org/obo/GAZ_00016863 -->

    <owl:NamedIndividual rdf:about="http://purl.obolibrary.org/obo/GAZ_00016863">
        <rdf:type rdf:resource="http://purl.obolibrary.org/obo/ENVO_00000222"/>
        <obo:RO_0001025 rdf:resource="http://purl.obolibrary.org/obo/GAZ_00007182"/>
        <obo:IAO_0000115>A volcanic island that is the easternmost island of the Louisiade Archipelago, which itself is part of the Milne Bay Province of Papua New Guinea.</obo:IAO_0000115>
        <oboInOwl:hasOBONamespace>GAZ</oboInOwl:hasOBONamespace>
        <oboInOwl:id>GAZ:00016863</oboInOwl:id>
        <rdfs:label>Rossel Island</rdfs:label>
    </owl:NamedIndividual>
    


    <!-- http://purl.obolibrary.org/obo/GAZ_00016864 -->

    <owl:NamedIndividual rdf:about="http://purl.obolibrary.org/obo/GAZ_00016864">
        <obo:RO_0001025 rdf:resource="http://purl.obolibrary.org/obo/GAZ_00007183"/>
        <oboInOwl:hasOBONamespace>GAZ</oboInOwl:hasOBONamespace>
        <oboInOwl:id>GAZ:00016864</oboInOwl:id>
        <rdfs:label>Kaileuna Island</rdfs:label>
    </owl:NamedIndividual>
    


    <!-- http://purl.obolibrary.org/obo/GAZ_00016865 -->

    <owl:NamedIndividual rdf:about="http://purl.obolibrary.org/obo/GAZ_00016865">
        <obo:RO_0001025 rdf:resource="http://purl.obolibrary.org/obo/GAZ_00007183"/>
        <oboInOwl:hasOBONamespace>GAZ</oboInOwl:hasOBONamespace>
        <oboInOwl:id>GAZ:00016865</oboInOwl:id>
        <rdfs:label>Vakuta Island</rdfs:label>
    </owl:NamedIndividual>
    


    <!-- http://purl.obolibrary.org/obo/GAZ_00016866 -->

    <owl:NamedIndividual rdf:about="http://purl.obolibrary.org/obo/GAZ_00016866">
        <obo:RO_0001025 rdf:resource="http://purl.obolibrary.org/obo/GAZ_00007183"/>
        <oboInOwl:hasOBONamespace>GAZ</oboInOwl:hasOBONamespace>
        <oboInOwl:id>GAZ:00016866</oboInOwl:id>
        <rdfs:label>Kitava Island</rdfs:label>
    </owl:NamedIndividual>
    


    <!-- http://purl.obolibrary.org/obo/GAZ_00016867 -->

    <owl:NamedIndividual rdf:about="http://purl.obolibrary.org/obo/GAZ_00016867">
        <obo:RO_0001025 rdf:resource="http://purl.obolibrary.org/obo/GAZ_00007183"/>
        <oboInOwl:hasOBONamespace>GAZ</oboInOwl:hasOBONamespace>
        <oboInOwl:id>GAZ:00016867</oboInOwl:id>
        <rdfs:label>Bolanga Island</rdfs:label>
    </owl:NamedIndividual>
    


    <!-- http://purl.obolibrary.org/obo/GAZ_00016868 -->

    <owl:NamedIndividual rdf:about="http://purl.obolibrary.org/obo/GAZ_00016868">
        <obo:RO_0001025 rdf:resource="http://purl.obolibrary.org/obo/GAZ_00007183"/>
        <oboInOwl:hasOBONamespace>GAZ</oboInOwl:hasOBONamespace>
        <oboInOwl:id>GAZ:00016868</oboInOwl:id>
        <rdfs:label>Tuma Island</rdfs:label>
    </owl:NamedIndividual>
    


    <!-- http://purl.obolibrary.org/obo/GAZ_00016869 -->

    <owl:NamedIndividual rdf:about="http://purl.obolibrary.org/obo/GAZ_00016869">
        <obo:RO_0001025 rdf:resource="http://purl.obolibrary.org/obo/GAZ_00007183"/>
        <oboInOwl:hasOBONamespace>GAZ</oboInOwl:hasOBONamespace>
        <oboInOwl:id>GAZ:00016869</oboInOwl:id>
        <rdfs:label>Kadai Island</rdfs:label>
    </owl:NamedIndividual>
    


    <!-- http://purl.obolibrary.org/obo/GAZ_00016870 -->

    <owl:NamedIndividual rdf:about="http://purl.obolibrary.org/obo/GAZ_00016870">
        <obo:RO_0001025 rdf:resource="http://purl.obolibrary.org/obo/GAZ_00007183"/>
        <oboInOwl:hasOBONamespace>GAZ</oboInOwl:hasOBONamespace>
        <oboInOwl:id>GAZ:00016870</oboInOwl:id>
        <rdfs:label>Munuwata Island</rdfs:label>
    </owl:NamedIndividual>
    


    <!-- http://purl.obolibrary.org/obo/GAZ_00016871 -->

    <owl:NamedIndividual rdf:about="http://purl.obolibrary.org/obo/GAZ_00016871">
        <obo:RO_0001025 rdf:resource="http://purl.obolibrary.org/obo/GAZ_00007183"/>
        <oboInOwl:hasOBONamespace>GAZ</oboInOwl:hasOBONamespace>
        <oboInOwl:id>GAZ:00016871</oboInOwl:id>
        <rdfs:label>Nubiam Island</rdfs:label>
    </owl:NamedIndividual>
    


    <!-- http://purl.obolibrary.org/obo/GAZ_00016872 -->

    <owl:NamedIndividual rdf:about="http://purl.obolibrary.org/obo/GAZ_00016872">
        <obo:RO_0001025 rdf:resource="http://purl.obolibrary.org/obo/GAZ_00007183"/>
        <oboInOwl:hasOBONamespace>GAZ</oboInOwl:hasOBONamespace>
        <oboInOwl:id>GAZ:00016872</oboInOwl:id>
        <rdfs:label>Labi Island</rdfs:label>
    </owl:NamedIndividual>
    


    <!-- http://purl.obolibrary.org/obo/GAZ_00016873 -->

    <owl:NamedIndividual rdf:about="http://purl.obolibrary.org/obo/GAZ_00016873">
        <obo:RO_0001025 rdf:resource="http://purl.obolibrary.org/obo/GAZ_00007183"/>
        <oboInOwl:hasOBONamespace>GAZ</oboInOwl:hasOBONamespace>
        <oboInOwl:id>GAZ:00016873</oboInOwl:id>
        <rdfs:label>Muwo Island</rdfs:label>
    </owl:NamedIndividual>
    


    <!-- http://purl.obolibrary.org/obo/GAZ_00016874 -->

    <owl:NamedIndividual rdf:about="http://purl.obolibrary.org/obo/GAZ_00016874">
        <obo:RO_0001025 rdf:resource="http://purl.obolibrary.org/obo/GAZ_00007183"/>
        <oboInOwl:hasOBONamespace>GAZ</oboInOwl:hasOBONamespace>
        <oboInOwl:id>GAZ:00016874</oboInOwl:id>
        <rdfs:label>Kibu Island</rdfs:label>
    </owl:NamedIndividual>
    


    <!-- http://purl.obolibrary.org/obo/GAZ_00016876 -->

    <owl:NamedIndividual rdf:about="http://purl.obolibrary.org/obo/GAZ_00016876">
        <obo:RO_0001025 rdf:resource="http://purl.obolibrary.org/obo/GAZ_00007183"/>
        <oboInOwl:hasOBONamespace>GAZ</oboInOwl:hasOBONamespace>
        <oboInOwl:id>GAZ:00016876</oboInOwl:id>
        <rdfs:label>Nulina Island</rdfs:label>
    </owl:NamedIndividual>
    


    <!-- http://purl.obolibrary.org/obo/GAZ_00016877 -->

    <owl:NamedIndividual rdf:about="http://purl.obolibrary.org/obo/GAZ_00016877">
        <obo:RO_0001025 rdf:resource="http://purl.obolibrary.org/obo/GAZ_00007183"/>
        <oboInOwl:hasOBONamespace>GAZ</oboInOwl:hasOBONamespace>
        <oboInOwl:id>GAZ:00016877</oboInOwl:id>
        <rdfs:label>Bomapau Island</rdfs:label>
    </owl:NamedIndividual>
    


    <!-- http://purl.obolibrary.org/obo/GAZ_00016878 -->

    <owl:NamedIndividual rdf:about="http://purl.obolibrary.org/obo/GAZ_00016878">
        <obo:RO_0001025 rdf:resource="http://purl.obolibrary.org/obo/GAZ_00007183"/>
        <oboInOwl:hasOBONamespace>GAZ</oboInOwl:hasOBONamespace>
        <oboInOwl:id>GAZ:00016878</oboInOwl:id>
        <rdfs:label>Simlindan Island</rdfs:label>
    </owl:NamedIndividual>
    


    <!-- http://purl.obolibrary.org/obo/GAZ_00022333 -->

    <owl:NamedIndividual rdf:about="http://purl.obolibrary.org/obo/GAZ_00022333">
        <rdf:type rdf:resource="http://purl.obolibrary.org/obo/ENVO_00000004"/>
        <obo:RO_0001025 rdf:resource="http://purl.obolibrary.org/obo/GAZ_00012657"/>
        <obo:IAO_0000115>A district of Central Province, Papua New Guinea.</obo:IAO_0000115>
        <oboInOwl:hasOBONamespace>GAZ</oboInOwl:hasOBONamespace>
        <oboInOwl:id>GAZ:00022333</oboInOwl:id>
        <rdfs:label>Kairuku-Hiri District</rdfs:label>
    </owl:NamedIndividual>
    


    <!-- http://purl.obolibrary.org/obo/GAZ_00022334 -->

    <owl:NamedIndividual rdf:about="http://purl.obolibrary.org/obo/GAZ_00022334">
        <rdf:type rdf:resource="http://purl.obolibrary.org/obo/ENVO_00000004"/>
        <obo:RO_0001025 rdf:resource="http://purl.obolibrary.org/obo/GAZ_00012657"/>
        <obo:IAO_0000115>A district of Central Province, Papua New Guinea.</obo:IAO_0000115>
        <oboInOwl:hasOBONamespace>GAZ</oboInOwl:hasOBONamespace>
        <oboInOwl:id>GAZ:00022334</oboInOwl:id>
        <rdfs:label>Rigo District</rdfs:label>
    </owl:NamedIndividual>
    


    <!-- http://purl.obolibrary.org/obo/GAZ_00022335 -->

    <owl:NamedIndividual rdf:about="http://purl.obolibrary.org/obo/GAZ_00022335">
        <rdf:type rdf:resource="http://purl.obolibrary.org/obo/ENVO_00000004"/>
        <obo:RO_0001025 rdf:resource="http://purl.obolibrary.org/obo/GAZ_00012657"/>
        <obo:IAO_0000115>A district of Central Province, Papua New Guinea.</obo:IAO_0000115>
        <oboInOwl:hasOBONamespace>GAZ</oboInOwl:hasOBONamespace>
        <oboInOwl:id>GAZ:00022335</oboInOwl:id>
        <rdfs:label>Abau District</rdfs:label>
    </owl:NamedIndividual>
    


    <!-- http://purl.obolibrary.org/obo/GAZ_00022336 -->

    <owl:NamedIndividual rdf:about="http://purl.obolibrary.org/obo/GAZ_00022336">
        <rdf:type rdf:resource="http://purl.obolibrary.org/obo/ENVO_00000004"/>
        <obo:RO_0001025 rdf:resource="http://purl.obolibrary.org/obo/GAZ_00012657"/>
        <obo:IAO_0000115>A district of Central Province, Papua New Guinea.</obo:IAO_0000115>
        <oboInOwl:hasOBONamespace>GAZ</oboInOwl:hasOBONamespace>
        <oboInOwl:id>GAZ:00022336</oboInOwl:id>
        <rdfs:label>Goilala District</rdfs:label>
    </owl:NamedIndividual>
    


    <!-- http://purl.obolibrary.org/obo/GAZ_00022337 -->

    <owl:NamedIndividual rdf:about="http://purl.obolibrary.org/obo/GAZ_00022337">
        <obo:RO_0001025 rdf:resource="http://purl.obolibrary.org/obo/GAZ_00010064"/>
        <oboInOwl:hasOBONamespace>GAZ</oboInOwl:hasOBONamespace>
        <oboInOwl:id>GAZ:00022337</oboInOwl:id>
        <rdfs:label>Kainantu District</rdfs:label>
    </owl:NamedIndividual>
    


    <!-- http://purl.obolibrary.org/obo/GAZ_00022338 -->

    <owl:NamedIndividual rdf:about="http://purl.obolibrary.org/obo/GAZ_00022338">
        <obo:RO_0001025 rdf:resource="http://purl.obolibrary.org/obo/GAZ_00010064"/>
        <oboInOwl:hasOBONamespace>GAZ</oboInOwl:hasOBONamespace>
        <oboInOwl:id>GAZ:00022338</oboInOwl:id>
        <rdfs:label>Obura-Wonenara District</rdfs:label>
    </owl:NamedIndividual>
    


    <!-- http://purl.obolibrary.org/obo/GAZ_00022339 -->

    <owl:NamedIndividual rdf:about="http://purl.obolibrary.org/obo/GAZ_00022339">
        <obo:RO_0001025 rdf:resource="http://purl.obolibrary.org/obo/GAZ_00010064"/>
        <oboInOwl:hasOBONamespace>GAZ</oboInOwl:hasOBONamespace>
        <oboInOwl:id>GAZ:00022339</oboInOwl:id>
        <rdfs:label>Unggai-Benna District</rdfs:label>
    </owl:NamedIndividual>
    


    <!-- http://purl.obolibrary.org/obo/GAZ_00022340 -->

    <owl:NamedIndividual rdf:about="http://purl.obolibrary.org/obo/GAZ_00022340">
        <obo:RO_0001025 rdf:resource="http://purl.obolibrary.org/obo/GAZ_00010064"/>
        <oboInOwl:hasOBONamespace>GAZ</oboInOwl:hasOBONamespace>
        <oboInOwl:id>GAZ:00022340</oboInOwl:id>
        <rdfs:label>Okapa District</rdfs:label>
    </owl:NamedIndividual>
    


    <!-- http://purl.obolibrary.org/obo/GAZ_00022341 -->

    <owl:NamedIndividual rdf:about="http://purl.obolibrary.org/obo/GAZ_00022341">
        <obo:RO_0001025 rdf:resource="http://purl.obolibrary.org/obo/GAZ_00010064"/>
        <oboInOwl:hasOBONamespace>GAZ</oboInOwl:hasOBONamespace>
        <oboInOwl:id>GAZ:00022341</oboInOwl:id>
        <rdfs:label>Goroka District</rdfs:label>
    </owl:NamedIndividual>
    


    <!-- http://purl.obolibrary.org/obo/GAZ_00022342 -->

    <owl:NamedIndividual rdf:about="http://purl.obolibrary.org/obo/GAZ_00022342">
        <obo:RO_0001025 rdf:resource="http://purl.obolibrary.org/obo/GAZ_00010064"/>
        <oboInOwl:hasOBONamespace>GAZ</oboInOwl:hasOBONamespace>
        <oboInOwl:id>GAZ:00022342</oboInOwl:id>
        <rdfs:label>Lufa District</rdfs:label>
    </owl:NamedIndividual>
    


    <!-- http://purl.obolibrary.org/obo/GAZ_00022343 -->

    <owl:NamedIndividual rdf:about="http://purl.obolibrary.org/obo/GAZ_00022343">
        <obo:RO_0001025 rdf:resource="http://purl.obolibrary.org/obo/GAZ_00010064"/>
        <oboInOwl:hasOBONamespace>GAZ</oboInOwl:hasOBONamespace>
        <oboInOwl:id>GAZ:00022343</oboInOwl:id>
        <rdfs:label>Daulo District</rdfs:label>
    </owl:NamedIndividual>
    


    <!-- http://purl.obolibrary.org/obo/GAZ_00022344 -->

    <owl:NamedIndividual rdf:about="http://purl.obolibrary.org/obo/GAZ_00022344">
        <obo:RO_0001025 rdf:resource="http://purl.obolibrary.org/obo/GAZ_00010064"/>
        <oboInOwl:hasOBONamespace>GAZ</oboInOwl:hasOBONamespace>
        <oboInOwl:id>GAZ:00022344</oboInOwl:id>
        <rdfs:label>Henganofi District</rdfs:label>
    </owl:NamedIndividual>
    


    <!-- http://purl.obolibrary.org/obo/GAZ_00022345 -->

    <owl:NamedIndividual rdf:about="http://purl.obolibrary.org/obo/GAZ_00022345">
        <rdf:type rdf:resource="http://purl.obolibrary.org/obo/ENVO_00000004"/>
        <obo:RO_0001025 rdf:resource="http://purl.obolibrary.org/obo/GAZ_00005192"/>
        <obo:IAO_0000115>A district of East New Britain Province, Papua New Guinea.</obo:IAO_0000115>
        <oboInOwl:hasOBONamespace>GAZ</oboInOwl:hasOBONamespace>
        <oboInOwl:id>GAZ:00022345</oboInOwl:id>
        <rdfs:label>Pomio District</rdfs:label>
    </owl:NamedIndividual>
    


    <!-- http://purl.obolibrary.org/obo/GAZ_00022346 -->

    <owl:NamedIndividual rdf:about="http://purl.obolibrary.org/obo/GAZ_00022346">
        <rdf:type rdf:resource="http://purl.obolibrary.org/obo/ENVO_00000004"/>
        <obo:RO_0001025 rdf:resource="http://purl.obolibrary.org/obo/GAZ_00005192"/>
        <obo:IAO_0000115>A district of East New Britain Province, Papua New Guinea.</obo:IAO_0000115>
        <oboInOwl:hasOBONamespace>GAZ</oboInOwl:hasOBONamespace>
        <oboInOwl:id>GAZ:00022346</oboInOwl:id>
        <rdfs:label>Rabaul District</rdfs:label>
    </owl:NamedIndividual>
    


    <!-- http://purl.obolibrary.org/obo/GAZ_00022347 -->

    <owl:NamedIndividual rdf:about="http://purl.obolibrary.org/obo/GAZ_00022347">
        <rdf:type rdf:resource="http://purl.obolibrary.org/obo/ENVO_00000004"/>
        <obo:RO_0001025 rdf:resource="http://purl.obolibrary.org/obo/GAZ_00005192"/>
        <obo:IAO_0000115>A district of East New Britain Province, Papua New Guinea.</obo:IAO_0000115>
        <oboInOwl:hasOBONamespace>GAZ</oboInOwl:hasOBONamespace>
        <oboInOwl:id>GAZ:00022347</oboInOwl:id>
        <rdfs:label>Kokopo District</rdfs:label>
    </owl:NamedIndividual>
    


    <!-- http://purl.obolibrary.org/obo/GAZ_00022348 -->

    <owl:NamedIndividual rdf:about="http://purl.obolibrary.org/obo/GAZ_00022348">
        <rdf:type rdf:resource="http://purl.obolibrary.org/obo/ENVO_00000004"/>
        <obo:RO_0001025 rdf:resource="http://purl.obolibrary.org/obo/GAZ_00005192"/>
        <obo:IAO_0000115>A district of East New Britain Province, Papua New Guinea.</obo:IAO_0000115>
        <oboInOwl:hasOBONamespace>GAZ</oboInOwl:hasOBONamespace>
        <oboInOwl:id>GAZ:00022348</oboInOwl:id>
        <rdfs:label>Gazelle District</rdfs:label>
    </owl:NamedIndividual>
    


    <!-- http://purl.obolibrary.org/obo/GAZ_00022349 -->

    <owl:NamedIndividual rdf:about="http://purl.obolibrary.org/obo/GAZ_00022349">
        <rdf:type rdf:resource="http://purl.obolibrary.org/obo/ENVO_00000004"/>
        <obo:RO_0001025 rdf:resource="http://purl.obolibrary.org/obo/GAZ_00005266"/>
        <obo:IAO_0000115>A district of East Sepik Province, Papua New Guinea.</obo:IAO_0000115>
        <oboInOwl:hasOBONamespace>GAZ</oboInOwl:hasOBONamespace>
        <oboInOwl:id>GAZ:00022349</oboInOwl:id>
        <rdfs:label>Angoram District</rdfs:label>
    </owl:NamedIndividual>
    


    <!-- http://purl.obolibrary.org/obo/GAZ_00022350 -->

    <owl:NamedIndividual rdf:about="http://purl.obolibrary.org/obo/GAZ_00022350">
        <rdf:type rdf:resource="http://purl.obolibrary.org/obo/ENVO_00000004"/>
        <obo:RO_0001025 rdf:resource="http://purl.obolibrary.org/obo/GAZ_00005266"/>
        <obo:IAO_0000115>A district of East Sepik Province, Papua New Guinea.</obo:IAO_0000115>
        <oboInOwl:hasOBONamespace>GAZ</oboInOwl:hasOBONamespace>
        <oboInOwl:id>GAZ:00022350</oboInOwl:id>
        <rdfs:label>Ambunti-Dreikikir District</rdfs:label>
    </owl:NamedIndividual>
    


    <!-- http://purl.obolibrary.org/obo/GAZ_00022351 -->

    <owl:NamedIndividual rdf:about="http://purl.obolibrary.org/obo/GAZ_00022351">
        <rdf:type rdf:resource="http://purl.obolibrary.org/obo/ENVO_00000004"/>
        <obo:RO_0001025 rdf:resource="http://purl.obolibrary.org/obo/GAZ_00005266"/>
        <obo:IAO_0000115>A district of East Sepik Province, Papua New Guinea.</obo:IAO_0000115>
        <oboInOwl:hasOBONamespace>GAZ</oboInOwl:hasOBONamespace>
        <oboInOwl:id>GAZ:00022351</oboInOwl:id>
        <rdfs:label>Wewak District</rdfs:label>
    </owl:NamedIndividual>
    


    <!-- http://purl.obolibrary.org/obo/GAZ_00022352 -->

    <owl:NamedIndividual rdf:about="http://purl.obolibrary.org/obo/GAZ_00022352">
        <rdf:type rdf:resource="http://purl.obolibrary.org/obo/ENVO_00000004"/>
        <obo:RO_0001025 rdf:resource="http://purl.obolibrary.org/obo/GAZ_00005266"/>
        <obo:IAO_0000115>A district of East Sepik Province, Papua New Guinea.</obo:IAO_0000115>
        <oboInOwl:hasOBONamespace>GAZ</oboInOwl:hasOBONamespace>
        <oboInOwl:id>GAZ:00022352</oboInOwl:id>
        <rdfs:label>Yangoru-Saussia District</rdfs:label>
    </owl:NamedIndividual>
    


    <!-- http://purl.obolibrary.org/obo/GAZ_00022353 -->

    <owl:NamedIndividual rdf:about="http://purl.obolibrary.org/obo/GAZ_00022353">
        <rdf:type rdf:resource="http://purl.obolibrary.org/obo/ENVO_00000004"/>
        <obo:RO_0001025 rdf:resource="http://purl.obolibrary.org/obo/GAZ_00005266"/>
        <obo:IAO_0000115>A district of East Sepik Province, Papua New Guinea.</obo:IAO_0000115>
        <oboInOwl:hasOBONamespace>GAZ</oboInOwl:hasOBONamespace>
        <oboInOwl:id>GAZ:00022353</oboInOwl:id>
        <rdfs:label>Wosera-Gawi District</rdfs:label>
    </owl:NamedIndividual>
    


    <!-- http://purl.obolibrary.org/obo/GAZ_00022354 -->

    <owl:NamedIndividual rdf:about="http://purl.obolibrary.org/obo/GAZ_00022354">
        <rdf:type rdf:resource="http://purl.obolibrary.org/obo/ENVO_00000004"/>
        <obo:RO_0001025 rdf:resource="http://purl.obolibrary.org/obo/GAZ_00005266"/>
        <obo:IAO_0000115>A district of East Sepik Province, Papua New Guinea.</obo:IAO_0000115>
        <oboInOwl:hasOBONamespace>GAZ</oboInOwl:hasOBONamespace>
        <oboInOwl:id>GAZ:00022354</oboInOwl:id>
        <rdfs:label>Maprik District</rdfs:label>
    </owl:NamedIndividual>
    


    <!-- http://purl.obolibrary.org/obo/GAZ_00022355 -->

    <owl:NamedIndividual rdf:about="http://purl.obolibrary.org/obo/GAZ_00022355">
        <rdf:type rdf:resource="http://purl.obolibrary.org/obo/ENVO_00000004"/>
        <obo:RO_0001025 rdf:resource="http://purl.obolibrary.org/obo/GAZ_00012659"/>
        <obo:IAO_0000115>A district of Gulf Province, Papua New Guinea.</obo:IAO_0000115>
        <oboInOwl:hasOBONamespace>GAZ</oboInOwl:hasOBONamespace>
        <oboInOwl:id>GAZ:00022355</oboInOwl:id>
        <rdfs:label>Kerema District</rdfs:label>
    </owl:NamedIndividual>
    


    <!-- http://purl.obolibrary.org/obo/GAZ_00022356 -->

    <owl:NamedIndividual rdf:about="http://purl.obolibrary.org/obo/GAZ_00022356">
        <rdf:type rdf:resource="http://purl.obolibrary.org/obo/ENVO_00000004"/>
        <obo:RO_0001025 rdf:resource="http://purl.obolibrary.org/obo/GAZ_00012660"/>
        <obo:IAO_0000115>A district of Enga Province, Papua New Guinea.</obo:IAO_0000115>
        <oboInOwl:hasOBONamespace>GAZ</oboInOwl:hasOBONamespace>
        <oboInOwl:id>GAZ:00022356</oboInOwl:id>
        <rdfs:label>Kompiam District</rdfs:label>
    </owl:NamedIndividual>
    


    <!-- http://purl.obolibrary.org/obo/GAZ_00022357 -->

    <owl:NamedIndividual rdf:about="http://purl.obolibrary.org/obo/GAZ_00022357">
        <rdf:type rdf:resource="http://purl.obolibrary.org/obo/ENVO_00000004"/>
        <obo:RO_0001025 rdf:resource="http://purl.obolibrary.org/obo/GAZ_00012660"/>
        <obo:IAO_0000115>A district of Enga Province, Papua New Guinea.</obo:IAO_0000115>
        <oboInOwl:hasOBONamespace>GAZ</oboInOwl:hasOBONamespace>
        <oboInOwl:id>GAZ:00022357</oboInOwl:id>
        <rdfs:label>Kandep District</rdfs:label>
    </owl:NamedIndividual>
    


    <!-- http://purl.obolibrary.org/obo/GAZ_00022358 -->

    <owl:NamedIndividual rdf:about="http://purl.obolibrary.org/obo/GAZ_00022358">
        <rdf:type rdf:resource="http://purl.obolibrary.org/obo/ENVO_00000004"/>
        <obo:RO_0001025 rdf:resource="http://purl.obolibrary.org/obo/GAZ_00012660"/>
        <obo:IAO_0000115>A district of Enga Province, Papua New Guinea.</obo:IAO_0000115>
        <oboInOwl:hasOBONamespace>GAZ</oboInOwl:hasOBONamespace>
        <oboInOwl:id>GAZ:00022358</oboInOwl:id>
        <rdfs:label>Lagaip-Porgera District</rdfs:label>
    </owl:NamedIndividual>
    


    <!-- http://purl.obolibrary.org/obo/GAZ_00022359 -->

    <owl:NamedIndividual rdf:about="http://purl.obolibrary.org/obo/GAZ_00022359">
        <rdf:type rdf:resource="http://purl.obolibrary.org/obo/ENVO_00000004"/>
        <obo:RO_0001025 rdf:resource="http://purl.obolibrary.org/obo/GAZ_00012660"/>
        <obo:IAO_0000115>A district of Enga Province, Papua New Guinea.</obo:IAO_0000115>
        <oboInOwl:hasOBONamespace>GAZ</oboInOwl:hasOBONamespace>
        <oboInOwl:id>GAZ:00022359</oboInOwl:id>
        <rdfs:label>Wabag District</rdfs:label>
    </owl:NamedIndividual>
    


    <!-- http://purl.obolibrary.org/obo/GAZ_00022360 -->

    <owl:NamedIndividual rdf:about="http://purl.obolibrary.org/obo/GAZ_00022360">
        <rdf:type rdf:resource="http://purl.obolibrary.org/obo/ENVO_00000004"/>
        <obo:RO_0001025 rdf:resource="http://purl.obolibrary.org/obo/GAZ_00012659"/>
        <obo:IAO_0000115>A district of Gulf Province, Papua New Guinea.</obo:IAO_0000115>
        <oboInOwl:hasOBONamespace>GAZ</oboInOwl:hasOBONamespace>
        <oboInOwl:id>GAZ:00022360</oboInOwl:id>
        <rdfs:label>Kikori District</rdfs:label>
    </owl:NamedIndividual>
    


    <!-- http://purl.obolibrary.org/obo/GAZ_00022361 -->

    <owl:NamedIndividual rdf:about="http://purl.obolibrary.org/obo/GAZ_00022361">
        <rdf:type rdf:resource="http://purl.obolibrary.org/obo/ENVO_00000004"/>
        <obo:RO_0001025 rdf:resource="http://purl.obolibrary.org/obo/GAZ_00005198"/>
        <obo:IAO_0000115>A district of Madang Province, Papua New Guinea.</obo:IAO_0000115>
        <oboInOwl:hasOBONamespace>GAZ</oboInOwl:hasOBONamespace>
        <oboInOwl:id>GAZ:00022361</oboInOwl:id>
        <rdfs:label>Bogia District</rdfs:label>
    </owl:NamedIndividual>
    


    <!-- http://purl.obolibrary.org/obo/GAZ_00022362 -->

    <owl:NamedIndividual rdf:about="http://purl.obolibrary.org/obo/GAZ_00022362">
        <rdf:type rdf:resource="http://purl.obolibrary.org/obo/ENVO_00000004"/>
        <obo:RO_0001025 rdf:resource="http://purl.obolibrary.org/obo/GAZ_00005198"/>
        <obo:IAO_0000115>A district of Madang Province, Papua New Guinea.</obo:IAO_0000115>
        <oboInOwl:hasOBONamespace>GAZ</oboInOwl:hasOBONamespace>
        <oboInOwl:id>GAZ:00022362</oboInOwl:id>
        <rdfs:label>Sumkar District</rdfs:label>
    </owl:NamedIndividual>
    


    <!-- http://purl.obolibrary.org/obo/GAZ_00022363 -->

    <owl:NamedIndividual rdf:about="http://purl.obolibrary.org/obo/GAZ_00022363">
        <rdf:type rdf:resource="http://purl.obolibrary.org/obo/ENVO_00000004"/>
        <obo:RO_0001025 rdf:resource="http://purl.obolibrary.org/obo/GAZ_00005198"/>
        <obo:IAO_0000115>A district of Madang Province, Papua New Guinea.</obo:IAO_0000115>
        <oboInOwl:hasOBONamespace>GAZ</oboInOwl:hasOBONamespace>
        <oboInOwl:id>GAZ:00022363</oboInOwl:id>
        <rdfs:label>Usino Bundi District</rdfs:label>
    </owl:NamedIndividual>
    


    <!-- http://purl.obolibrary.org/obo/GAZ_00022364 -->

    <owl:NamedIndividual rdf:about="http://purl.obolibrary.org/obo/GAZ_00022364">
        <rdf:type rdf:resource="http://purl.obolibrary.org/obo/ENVO_00000004"/>
        <obo:RO_0001025 rdf:resource="http://purl.obolibrary.org/obo/GAZ_00005198"/>
        <obo:IAO_0000115>A district of Madang Province, Papua New Guinea.</obo:IAO_0000115>
        <oboInOwl:hasOBONamespace>GAZ</oboInOwl:hasOBONamespace>
        <oboInOwl:id>GAZ:00022364</oboInOwl:id>
        <rdfs:label>Rai Coast District</rdfs:label>
    </owl:NamedIndividual>
    


    <!-- http://purl.obolibrary.org/obo/GAZ_00022365 -->

    <owl:NamedIndividual rdf:about="http://purl.obolibrary.org/obo/GAZ_00022365">
        <rdf:type rdf:resource="http://purl.obolibrary.org/obo/ENVO_00000004"/>
        <obo:RO_0001025 rdf:resource="http://purl.obolibrary.org/obo/GAZ_00005198"/>
        <obo:IAO_0000115>A district of Madang Province, Papua New Guinea.</obo:IAO_0000115>
        <oboInOwl:hasOBONamespace>GAZ</oboInOwl:hasOBONamespace>
        <oboInOwl:id>GAZ:00022365</oboInOwl:id>
        <rdfs:label>Madang District</rdfs:label>
    </owl:NamedIndividual>
    


    <!-- http://purl.obolibrary.org/obo/GAZ_00022366 -->

    <owl:NamedIndividual rdf:about="http://purl.obolibrary.org/obo/GAZ_00022366">
        <rdf:type rdf:resource="http://purl.obolibrary.org/obo/ENVO_00000004"/>
        <obo:RO_0001025 rdf:resource="http://purl.obolibrary.org/obo/GAZ_00005198"/>
        <obo:IAO_0000115>A district of Madang Province, Papua New Guinea.</obo:IAO_0000115>
        <oboInOwl:hasOBONamespace>GAZ</oboInOwl:hasOBONamespace>
        <oboInOwl:id>GAZ:00022366</oboInOwl:id>
        <rdfs:label>Middle Ramu District</rdfs:label>
    </owl:NamedIndividual>
    


    <!-- http://purl.obolibrary.org/obo/GAZ_00022367 -->

    <owl:NamedIndividual rdf:about="http://purl.obolibrary.org/obo/GAZ_00022367">
        <obo:RO_0001025 rdf:resource="http://purl.obolibrary.org/obo/GAZ_00022341"/>
        <oboInOwl:hasOBONamespace>GAZ</oboInOwl:hasOBONamespace>
        <oboInOwl:id>GAZ:00022367</oboInOwl:id>
        <rdfs:label>Goroka Rural Local-Level Government Area</rdfs:label>
    </owl:NamedIndividual>
    


    <!-- http://purl.obolibrary.org/obo/GAZ_00022368 -->

    <owl:NamedIndividual rdf:about="http://purl.obolibrary.org/obo/GAZ_00022368">
        <obo:RO_0001025 rdf:resource="http://purl.obolibrary.org/obo/GAZ_00022341"/>
        <oboInOwl:hasOBONamespace>GAZ</oboInOwl:hasOBONamespace>
        <oboInOwl:id>GAZ:00022368</oboInOwl:id>
        <rdfs:label>Goroka Urban Local-Level Government Area</rdfs:label>
    </owl:NamedIndividual>
    


    <!-- http://purl.obolibrary.org/obo/GAZ_00022369 -->

    <owl:NamedIndividual rdf:about="http://purl.obolibrary.org/obo/GAZ_00022369">
        <obo:RO_0001025 rdf:resource="http://purl.obolibrary.org/obo/GAZ_00022351"/>
        <obo:IAO_0000115>A Local-Level Government Area of Wewak District.</obo:IAO_0000115>
        <oboInOwl:hasOBONamespace>GAZ</oboInOwl:hasOBONamespace>
        <oboInOwl:id>GAZ:00022369</oboInOwl:id>
        <rdfs:label>Wewak Rural Local-Level Government Area</rdfs:label>
    </owl:NamedIndividual>
    


    <!-- http://purl.obolibrary.org/obo/GAZ_00022370 -->

    <owl:NamedIndividual rdf:about="http://purl.obolibrary.org/obo/GAZ_00022370">
        <obo:RO_0001025 rdf:resource="http://purl.obolibrary.org/obo/GAZ_00022351"/>
        <obo:IAO_0000115>A Local-Level Government Area of Wewak District.</obo:IAO_0000115>
        <oboInOwl:hasOBONamespace>GAZ</oboInOwl:hasOBONamespace>
        <oboInOwl:id>GAZ:00022370</oboInOwl:id>
        <rdfs:label>Wewak Urban Local-Level Government Area</rdfs:label>
    </owl:NamedIndividual>
    


    <!-- http://purl.obolibrary.org/obo/GAZ_00022371 -->

    <owl:NamedIndividual rdf:about="http://purl.obolibrary.org/obo/GAZ_00022371">
        <obo:RO_0001025 rdf:resource="http://purl.obolibrary.org/obo/GAZ_00022351"/>
        <obo:IAO_0000115>A Local-Level Government Area of Wewak District.</obo:IAO_0000115>
        <oboInOwl:hasOBONamespace>GAZ</oboInOwl:hasOBONamespace>
        <oboInOwl:id>GAZ:00022371</oboInOwl:id>
        <rdfs:label>Turubu Rural Local-Level Government Area</rdfs:label>
    </owl:NamedIndividual>
    


    <!-- http://purl.obolibrary.org/obo/GAZ_00022372 -->

    <owl:NamedIndividual rdf:about="http://purl.obolibrary.org/obo/GAZ_00022372">
        <obo:RO_0001025 rdf:resource="http://purl.obolibrary.org/obo/GAZ_00022351"/>
        <obo:IAO_0000115>A Local-Level Government Area of Wewak District.</obo:IAO_0000115>
        <oboInOwl:hasOBONamespace>GAZ</oboInOwl:hasOBONamespace>
        <oboInOwl:id>GAZ:00022372</oboInOwl:id>
        <rdfs:label>Wewak Islands Rural Local-Level Government Area</rdfs:label>
    </owl:NamedIndividual>
    


    <!-- http://purl.obolibrary.org/obo/GAZ_00022373 -->

    <owl:NamedIndividual rdf:about="http://purl.obolibrary.org/obo/GAZ_00022373">
        <obo:RO_0001025 rdf:resource="http://purl.obolibrary.org/obo/GAZ_00022351"/>
        <obo:IAO_0000115>A Local-Level Government Area of Wewak District.</obo:IAO_0000115>
        <oboInOwl:hasOBONamespace>GAZ</oboInOwl:hasOBONamespace>
        <oboInOwl:id>GAZ:00022373</oboInOwl:id>
        <rdfs:label>Boikin Dagua Rural Local-Level Government Area</rdfs:label>
    </owl:NamedIndividual>
    


    <!-- http://purl.obolibrary.org/obo/GAZ_00022374 -->

    <owl:NamedIndividual rdf:about="http://purl.obolibrary.org/obo/GAZ_00022374">
        <obo:RO_0001025 rdf:resource="http://purl.obolibrary.org/obo/GAZ_00022346"/>
        <obo:IAO_0000115>A Local-Level Government Area of Rabaul District.</obo:IAO_0000115>
        <oboInOwl:hasOBONamespace>GAZ</oboInOwl:hasOBONamespace>
        <oboInOwl:id>GAZ:00022374</oboInOwl:id>
        <rdfs:label>Balanataman Rural Local-Level Government Area</rdfs:label>
    </owl:NamedIndividual>
    


    <!-- http://purl.obolibrary.org/obo/GAZ_00022375 -->

    <owl:NamedIndividual rdf:about="http://purl.obolibrary.org/obo/GAZ_00022375">
        <obo:RO_0001025 rdf:resource="http://purl.obolibrary.org/obo/GAZ_00022346"/>
        <obo:IAO_0000115>A Local-Level Government Area of Rabaul District.</obo:IAO_0000115>
        <oboInOwl:hasOBONamespace>GAZ</oboInOwl:hasOBONamespace>
        <oboInOwl:id>GAZ:00022375</oboInOwl:id>
        <rdfs:label>Watom Island Rural Local-Level Government Area</rdfs:label>
    </owl:NamedIndividual>
    


    <!-- http://purl.obolibrary.org/obo/GAZ_00022376 -->

    <owl:NamedIndividual rdf:about="http://purl.obolibrary.org/obo/GAZ_00022376">
        <obo:RO_0001025 rdf:resource="http://purl.obolibrary.org/obo/GAZ_00022346"/>
        <obo:IAO_0000115>A Local-Level Government Area of Rabaul District.</obo:IAO_0000115>
        <oboInOwl:hasOBONamespace>GAZ</oboInOwl:hasOBONamespace>
        <oboInOwl:id>GAZ:00022376</oboInOwl:id>
        <rdfs:label>Kombiu Rural Local-Level Government Area</rdfs:label>
    </owl:NamedIndividual>
    


    <!-- http://purl.obolibrary.org/obo/GAZ_00022377 -->

    <owl:NamedIndividual rdf:about="http://purl.obolibrary.org/obo/GAZ_00022377">
        <obo:RO_0001025 rdf:resource="http://purl.obolibrary.org/obo/GAZ_00022346"/>
        <obo:IAO_0000115>A Local-Level Government Area of Rabaul District.</obo:IAO_0000115>
        <oboInOwl:hasOBONamespace>GAZ</oboInOwl:hasOBONamespace>
        <oboInOwl:id>GAZ:00022377</oboInOwl:id>
        <rdfs:label>Rabaul Urban Local-Level Government Area</rdfs:label>
    </owl:NamedIndividual>
    


    <!-- http://purl.obolibrary.org/obo/GAZ_00022378 -->

    <owl:NamedIndividual rdf:about="http://purl.obolibrary.org/obo/GAZ_00022378">
        <obo:RO_0001025 rdf:resource="http://purl.obolibrary.org/obo/GAZ_00012667"/>
        <obo:IAO_0000115>The single district of Manus Province, Papua New Guinea.</obo:IAO_0000115>
        <oboInOwl:hasOBONamespace>GAZ</oboInOwl:hasOBONamespace>
        <oboInOwl:id>GAZ:00022378</oboInOwl:id>
        <rdfs:label>Manus District</rdfs:label>
    </owl:NamedIndividual>
    


    <!-- http://purl.obolibrary.org/obo/GAZ_00022379 -->

    <owl:NamedIndividual rdf:about="http://purl.obolibrary.org/obo/GAZ_00022379">
        <rdf:type rdf:resource="http://purl.obolibrary.org/obo/ENVO_00000004"/>
        <obo:RO_0001025 rdf:resource="http://purl.obolibrary.org/obo/GAZ_00012666"/>
        <obo:IAO_0000115>A district of Milne Bay Province, Papua New Guinea.</obo:IAO_0000115>
        <oboInOwl:hasOBONamespace>GAZ</oboInOwl:hasOBONamespace>
        <oboInOwl:id>GAZ:00022379</oboInOwl:id>
        <rdfs:label>Samarai-Murua District</rdfs:label>
    </owl:NamedIndividual>
    


    <!-- http://purl.obolibrary.org/obo/GAZ_00022380 -->

    <owl:NamedIndividual rdf:about="http://purl.obolibrary.org/obo/GAZ_00022380">
        <rdf:type rdf:resource="http://purl.obolibrary.org/obo/ENVO_00000004"/>
        <obo:RO_0001025 rdf:resource="http://purl.obolibrary.org/obo/GAZ_00012666"/>
        <obo:IAO_0000115>A district of Milne Bay Province, Papua New Guinea.</obo:IAO_0000115>
        <oboInOwl:hasOBONamespace>GAZ</oboInOwl:hasOBONamespace>
        <oboInOwl:id>GAZ:00022380</oboInOwl:id>
        <rdfs:label>Esa&apos;ala District</rdfs:label>
    </owl:NamedIndividual>
    


    <!-- http://purl.obolibrary.org/obo/GAZ_00022381 -->

    <owl:NamedIndividual rdf:about="http://purl.obolibrary.org/obo/GAZ_00022381">
        <rdf:type rdf:resource="http://purl.obolibrary.org/obo/ENVO_00000004"/>
        <obo:RO_0001025 rdf:resource="http://purl.obolibrary.org/obo/GAZ_00012666"/>
        <obo:IAO_0000115>A district of Milne Bay Province, Papua New Guinea.</obo:IAO_0000115>
        <oboInOwl:hasOBONamespace>GAZ</oboInOwl:hasOBONamespace>
        <oboInOwl:id>GAZ:00022381</oboInOwl:id>
        <rdfs:label>Alotau District</rdfs:label>
    </owl:NamedIndividual>
    


    <!-- http://purl.obolibrary.org/obo/GAZ_00022382 -->

    <owl:NamedIndividual rdf:about="http://purl.obolibrary.org/obo/GAZ_00022382">
        <rdf:type rdf:resource="http://purl.obolibrary.org/obo/ENVO_00000004"/>
        <obo:RO_0001025 rdf:resource="http://purl.obolibrary.org/obo/GAZ_00012666"/>
        <obo:IAO_0000115>A district of Milne Bay Province, Papua New Guinea.</obo:IAO_0000115>
        <oboInOwl:hasOBONamespace>GAZ</oboInOwl:hasOBONamespace>
        <oboInOwl:id>GAZ:00022382</oboInOwl:id>
        <rdfs:label>Kiriwini-Goodenough District</rdfs:label>
    </owl:NamedIndividual>
    


    <!-- http://purl.obolibrary.org/obo/GAZ_00022383 -->

    <owl:NamedIndividual rdf:about="http://purl.obolibrary.org/obo/GAZ_00022383">
        <obo:RO_0001025 rdf:resource="http://purl.obolibrary.org/obo/GAZ_00007256"/>
        <obo:IAO_0000115>A Local-Level Government Area of Finschhafen District.</obo:IAO_0000115>
        <oboInOwl:hasOBONamespace>GAZ</oboInOwl:hasOBONamespace>
        <oboInOwl:id>GAZ:00022383</oboInOwl:id>
        <rdfs:label>Yabim-Mape Rural Local-Level Government Area</rdfs:label>
    </owl:NamedIndividual>
    


    <!-- http://purl.obolibrary.org/obo/GAZ_00022384 -->

    <owl:NamedIndividual rdf:about="http://purl.obolibrary.org/obo/GAZ_00022384">
        <obo:RO_0001025 rdf:resource="http://purl.obolibrary.org/obo/GAZ_00007256"/>
        <obo:IAO_0000115>A Local-Level Government Area of Finschhafen District.</obo:IAO_0000115>
        <oboInOwl:hasOBONamespace>GAZ</oboInOwl:hasOBONamespace>
        <oboInOwl:id>GAZ:00022384</oboInOwl:id>
        <rdfs:label>Burum-Kuat Rural Local-Level Government Area</rdfs:label>
    </owl:NamedIndividual>
    


    <!-- http://purl.obolibrary.org/obo/GAZ_00022385 -->

    <owl:NamedIndividual rdf:about="http://purl.obolibrary.org/obo/GAZ_00022385">
        <obo:RO_0001025 rdf:resource="http://purl.obolibrary.org/obo/GAZ_00007256"/>
        <obo:IAO_0000115>A Local-Level Government Area of Finschhafen District.</obo:IAO_0000115>
        <oboInOwl:hasOBONamespace>GAZ</oboInOwl:hasOBONamespace>
        <oboInOwl:id>GAZ:00022385</oboInOwl:id>
        <rdfs:label>Kotte Rural Local-Level Government Area</rdfs:label>
    </owl:NamedIndividual>
    


    <!-- http://purl.obolibrary.org/obo/GAZ_00022386 -->

    <owl:NamedIndividual rdf:about="http://purl.obolibrary.org/obo/GAZ_00022386">
        <obo:RO_0001025 rdf:resource="http://purl.obolibrary.org/obo/GAZ_00007256"/>
        <obo:IAO_0000115>A Local-Level Government Area of Finschhafen District.</obo:IAO_0000115>
        <oboInOwl:hasOBONamespace>GAZ</oboInOwl:hasOBONamespace>
        <oboInOwl:id>GAZ:00022386</oboInOwl:id>
        <rdfs:label>Hube Rural Local-Level Government Area</rdfs:label>
    </owl:NamedIndividual>
    


    <!-- http://purl.obolibrary.org/obo/GAZ_00022387 -->

    <owl:NamedIndividual rdf:about="http://purl.obolibrary.org/obo/GAZ_00022387">
        <obo:RO_0001025 rdf:resource="http://purl.obolibrary.org/obo/GAZ_00007256"/>
        <obo:IAO_0000115>A Local-Level Government Area of Finschhafen District.</obo:IAO_0000115>
        <oboInOwl:hasOBONamespace>GAZ</oboInOwl:hasOBONamespace>
        <oboInOwl:id>GAZ:00022387</oboInOwl:id>
        <rdfs:label>Finschafen Urban Local-Level Government Area</rdfs:label>
    </owl:NamedIndividual>
    


    <!-- http://purl.obolibrary.org/obo/GAZ_00022388 -->

    <owl:NamedIndividual rdf:about="http://purl.obolibrary.org/obo/GAZ_00022388">
        <rdf:type rdf:resource="http://purl.obolibrary.org/obo/ENVO_00000004"/>
        <obo:RO_0001025 rdf:resource="http://purl.obolibrary.org/obo/GAZ_00007255"/>
        <obo:IAO_0000115>A district of Morobe Province, Papua New Guinea.</obo:IAO_0000115>
        <oboInOwl:hasOBONamespace>GAZ</oboInOwl:hasOBONamespace>
        <oboInOwl:id>GAZ:00022388</oboInOwl:id>
        <rdfs:label>Bulolo District</rdfs:label>
    </owl:NamedIndividual>
    


    <!-- http://purl.obolibrary.org/obo/GAZ_00022389 -->

    <owl:NamedIndividual rdf:about="http://purl.obolibrary.org/obo/GAZ_00022389">
        <rdf:type rdf:resource="http://purl.obolibrary.org/obo/ENVO_00000004"/>
        <obo:RO_0001025 rdf:resource="http://purl.obolibrary.org/obo/GAZ_00007255"/>
        <obo:IAO_0000115>A district of Morobe Province, Papua New Guinea.</obo:IAO_0000115>
        <oboInOwl:hasOBONamespace>GAZ</oboInOwl:hasOBONamespace>
        <oboInOwl:id>GAZ:00022389</oboInOwl:id>
        <rdfs:label>Tewae-Siassi District</rdfs:label>
    </owl:NamedIndividual>
    


    <!-- http://purl.obolibrary.org/obo/GAZ_00022390 -->

    <owl:NamedIndividual rdf:about="http://purl.obolibrary.org/obo/GAZ_00022390">
        <rdf:type rdf:resource="http://purl.obolibrary.org/obo/ENVO_00000004"/>
        <obo:RO_0001025 rdf:resource="http://purl.obolibrary.org/obo/GAZ_00007255"/>
        <obo:IAO_0000115>A district of Morobe Province, Papua New Guinea.</obo:IAO_0000115>
        <oboInOwl:hasOBONamespace>GAZ</oboInOwl:hasOBONamespace>
        <oboInOwl:id>GAZ:00022390</oboInOwl:id>
        <rdfs:label>Kabwum District</rdfs:label>
    </owl:NamedIndividual>
    


    <!-- http://purl.obolibrary.org/obo/GAZ_00022391 -->

    <owl:NamedIndividual rdf:about="http://purl.obolibrary.org/obo/GAZ_00022391">
        <rdf:type rdf:resource="http://purl.obolibrary.org/obo/ENVO_00000004"/>
        <obo:RO_0001025 rdf:resource="http://purl.obolibrary.org/obo/GAZ_00007255"/>
        <obo:IAO_0000115>A district of Morobe Province, Papua New Guinea.</obo:IAO_0000115>
        <oboInOwl:hasOBONamespace>GAZ</oboInOwl:hasOBONamespace>
        <oboInOwl:id>GAZ:00022391</oboInOwl:id>
        <rdfs:label>Menyamya District</rdfs:label>
    </owl:NamedIndividual>
    


    <!-- http://purl.obolibrary.org/obo/GAZ_00022392 -->

    <owl:NamedIndividual rdf:about="http://purl.obolibrary.org/obo/GAZ_00022392">
        <rdf:type rdf:resource="http://purl.obolibrary.org/obo/ENVO_00000004"/>
        <obo:RO_0001025 rdf:resource="http://purl.obolibrary.org/obo/GAZ_00007255"/>
        <obo:IAO_0000115>A district of Morobe Province, Papua New Guinea.</obo:IAO_0000115>
        <oboInOwl:hasOBONamespace>GAZ</oboInOwl:hasOBONamespace>
        <oboInOwl:id>GAZ:00022392</oboInOwl:id>
        <rdfs:label>Lae District</rdfs:label>
    </owl:NamedIndividual>
    


    <!-- http://purl.obolibrary.org/obo/GAZ_00022393 -->

    <owl:NamedIndividual rdf:about="http://purl.obolibrary.org/obo/GAZ_00022393">
        <rdf:type rdf:resource="http://purl.obolibrary.org/obo/ENVO_00000004"/>
        <obo:RO_0001025 rdf:resource="http://purl.obolibrary.org/obo/GAZ_00007255"/>
        <obo:IAO_0000115>A district of Morobe Province, Papua New Guinea.</obo:IAO_0000115>
        <oboInOwl:hasOBONamespace>GAZ</oboInOwl:hasOBONamespace>
        <oboInOwl:id>GAZ:00022393</oboInOwl:id>
        <rdfs:label>Huon District</rdfs:label>
    </owl:NamedIndividual>
    


    <!-- http://purl.obolibrary.org/obo/GAZ_00022394 -->

    <owl:NamedIndividual rdf:about="http://purl.obolibrary.org/obo/GAZ_00022394">
        <rdf:type rdf:resource="http://purl.obolibrary.org/obo/ENVO_00000004"/>
        <obo:RO_0001025 rdf:resource="http://purl.obolibrary.org/obo/GAZ_00007255"/>
        <obo:IAO_0000115>A district of Morobe Province, Papua New Guinea.</obo:IAO_0000115>
        <oboInOwl:hasOBONamespace>GAZ</oboInOwl:hasOBONamespace>
        <oboInOwl:id>GAZ:00022394</oboInOwl:id>
        <rdfs:label>Nawae District</rdfs:label>
    </owl:NamedIndividual>
    


    <!-- http://purl.obolibrary.org/obo/GAZ_00022395 -->

    <owl:NamedIndividual rdf:about="http://purl.obolibrary.org/obo/GAZ_00022395">
        <rdf:type rdf:resource="http://purl.obolibrary.org/obo/ENVO_00000004"/>
        <obo:RO_0001025 rdf:resource="http://purl.obolibrary.org/obo/GAZ_00007255"/>
        <obo:IAO_0000115>A district of Morobe Province, Papua New Guinea.</obo:IAO_0000115>
        <oboInOwl:hasOBONamespace>GAZ</oboInOwl:hasOBONamespace>
        <oboInOwl:id>GAZ:00022395</oboInOwl:id>
        <rdfs:label>Markham District</rdfs:label>
    </owl:NamedIndividual>
    


    <!-- http://purl.obolibrary.org/obo/GAZ_00022396 -->

    <owl:NamedIndividual rdf:about="http://purl.obolibrary.org/obo/GAZ_00022396">
        <rdf:type rdf:resource="http://purl.obolibrary.org/obo/ENVO_00000004"/>
        <obo:RO_0001025 rdf:resource="http://purl.obolibrary.org/obo/GAZ_00005190"/>
        <obo:IAO_0000115>A district of New Ireland Province, Papua New Guinea. The district contains the northern part of the island of New Ireland, as well as New Hannover, and the St. Matthias Group.</obo:IAO_0000115>
        <oboInOwl:hasOBONamespace>GAZ</oboInOwl:hasOBONamespace>
        <oboInOwl:id>GAZ:00022396</oboInOwl:id>
        <rdfs:label>Kavieng District</rdfs:label>
    </owl:NamedIndividual>
    


    <!-- http://purl.obolibrary.org/obo/GAZ_00022397 -->

    <owl:NamedIndividual rdf:about="http://purl.obolibrary.org/obo/GAZ_00022397">
        <rdf:type rdf:resource="http://purl.obolibrary.org/obo/ENVO_00000004"/>
        <obo:RO_0001025 rdf:resource="http://purl.obolibrary.org/obo/GAZ_00005190"/>
        <obo:IAO_0000115>A district of New Ireland Province, Papua New Guinea. The district covers the southern part of the island of New Ireland, as well as the Tabar Group, the Lihir Group, the Tangga Group and the Feni Islands.</obo:IAO_0000115>
        <oboInOwl:hasOBONamespace>GAZ</oboInOwl:hasOBONamespace>
        <oboInOwl:id>GAZ:00022397</oboInOwl:id>
        <rdfs:label>Namatanai District</rdfs:label>
    </owl:NamedIndividual>
    


    <!-- http://purl.obolibrary.org/obo/GAZ_00022398 -->

    <owl:NamedIndividual rdf:about="http://purl.obolibrary.org/obo/GAZ_00022398">
        <obo:RO_0001025 rdf:resource="http://purl.obolibrary.org/obo/GAZ_00005193"/>
        <oboInOwl:hasOBONamespace>GAZ</oboInOwl:hasOBONamespace>
        <oboInOwl:id>GAZ:00022398</oboInOwl:id>
        <rdfs:label>New Ireland Group</rdfs:label>
    </owl:NamedIndividual>
    


    <!-- http://purl.obolibrary.org/obo/GAZ_00022399 -->

    <owl:NamedIndividual rdf:about="http://purl.obolibrary.org/obo/GAZ_00022399">
        <obo:RO_0001025 rdf:resource="http://purl.obolibrary.org/obo/GAZ_00022398"/>
        <obo:RO_0001025 rdf:resource="http://purl.obolibrary.org/obo/GAZ_00118103"/>
        <obo:IAO_0000115>An island in New Ireland Province, Papua New Guinea.</obo:IAO_0000115>
        <oboInOwl:hasOBONamespace>GAZ</oboInOwl:hasOBONamespace>
        <oboInOwl:id>GAZ:00022399</oboInOwl:id>
        <rdfs:label>Dyaul Island</rdfs:label>
    </owl:NamedIndividual>
    


    <!-- http://purl.obolibrary.org/obo/GAZ_00022400 -->

    <owl:NamedIndividual rdf:about="http://purl.obolibrary.org/obo/GAZ_00022400">
        <rdf:type rdf:resource="http://purl.obolibrary.org/obo/ENVO_00000004"/>
        <obo:RO_0001025 rdf:resource="http://purl.obolibrary.org/obo/GAZ_00005182"/>
        <obo:IAO_0000115>A district of North Solomons Province, Papua New Guinea.</obo:IAO_0000115>
        <oboInOwl:hasOBONamespace>GAZ</oboInOwl:hasOBONamespace>
        <oboInOwl:id>GAZ:00022400</oboInOwl:id>
        <rdfs:label>North Bougainville District</rdfs:label>
    </owl:NamedIndividual>
    


    <!-- http://purl.obolibrary.org/obo/GAZ_00022401 -->

    <owl:NamedIndividual rdf:about="http://purl.obolibrary.org/obo/GAZ_00022401">
        <obo:RO_0001025 rdf:resource="http://purl.obolibrary.org/obo/GAZ_00022403"/>
        <obo:IAO_0000115>A Local-Level Government Area of Central Bougainville District.</obo:IAO_0000115>
        <oboInOwl:hasOBONamespace>GAZ</oboInOwl:hasOBONamespace>
        <oboInOwl:id>GAZ:00022401</oboInOwl:id>
        <rdfs:label>Wakunai Rural Local-Level Government Area</rdfs:label>
    </owl:NamedIndividual>
    


    <!-- http://purl.obolibrary.org/obo/GAZ_00022402 -->

    <owl:NamedIndividual rdf:about="http://purl.obolibrary.org/obo/GAZ_00022402">
        <rdf:type rdf:resource="http://purl.obolibrary.org/obo/ENVO_00000004"/>
        <obo:RO_0001025 rdf:resource="http://purl.obolibrary.org/obo/GAZ_00005182"/>
        <obo:IAO_0000115>A district of North Solomons Province, Papua New Guinea.</obo:IAO_0000115>
        <oboInOwl:hasOBONamespace>GAZ</oboInOwl:hasOBONamespace>
        <oboInOwl:id>GAZ:00022402</oboInOwl:id>
        <rdfs:label>South Bougainville District</rdfs:label>
    </owl:NamedIndividual>
    


    <!-- http://purl.obolibrary.org/obo/GAZ_00022403 -->

    <owl:NamedIndividual rdf:about="http://purl.obolibrary.org/obo/GAZ_00022403">
        <rdf:type rdf:resource="http://purl.obolibrary.org/obo/ENVO_00000004"/>
        <obo:RO_0001025 rdf:resource="http://purl.obolibrary.org/obo/GAZ_00005182"/>
        <obo:IAO_0000115>A district of North Solomons Province, Papua New Guinea.</obo:IAO_0000115>
        <oboInOwl:hasOBONamespace>GAZ</oboInOwl:hasOBONamespace>
        <oboInOwl:id>GAZ:00022403</oboInOwl:id>
        <rdfs:label>Central Bougainville District</rdfs:label>
    </owl:NamedIndividual>
    


    <!-- http://purl.obolibrary.org/obo/GAZ_00022404 -->

    <owl:NamedIndividual rdf:about="http://purl.obolibrary.org/obo/GAZ_00022404">
        <obo:RO_0001025 rdf:resource="http://purl.obolibrary.org/obo/GAZ_00022403"/>
        <obo:IAO_0000115>A Local-Level Government Area of Central Bougainville District.</obo:IAO_0000115>
        <oboInOwl:hasOBONamespace>GAZ</oboInOwl:hasOBONamespace>
        <oboInOwl:id>GAZ:00022404</oboInOwl:id>
        <rdfs:label>Arawa Rural Local-Level Government Area</rdfs:label>
    </owl:NamedIndividual>
    


    <!-- http://purl.obolibrary.org/obo/GAZ_00022405 -->

    <owl:NamedIndividual rdf:about="http://purl.obolibrary.org/obo/GAZ_00022405">
        <obo:RO_0001025 rdf:resource="http://purl.obolibrary.org/obo/GAZ_00022402"/>
        <obo:IAO_0000115>A Local-Level Government Area of South Bougainville District.</obo:IAO_0000115>
        <oboInOwl:hasOBONamespace>GAZ</oboInOwl:hasOBONamespace>
        <oboInOwl:id>GAZ:00022405</oboInOwl:id>
        <rdfs:label>Bana Rural Local-Level Government Area</rdfs:label>
    </owl:NamedIndividual>
    


    <!-- http://purl.obolibrary.org/obo/GAZ_00022406 -->

    <owl:NamedIndividual rdf:about="http://purl.obolibrary.org/obo/GAZ_00022406">
        <obo:RO_0001025 rdf:resource="http://purl.obolibrary.org/obo/GAZ_00022402"/>
        <obo:IAO_0000115>A Local-Level Government Area of South Bougainville District.</obo:IAO_0000115>
        <oboInOwl:hasOBONamespace>GAZ</oboInOwl:hasOBONamespace>
        <oboInOwl:id>GAZ:00022406</oboInOwl:id>
        <rdfs:label>Buin Rural Local-Level Government Area</rdfs:label>
    </owl:NamedIndividual>
    


    <!-- http://purl.obolibrary.org/obo/GAZ_00022407 -->

    <owl:NamedIndividual rdf:about="http://purl.obolibrary.org/obo/GAZ_00022407">
        <obo:RO_0001025 rdf:resource="http://purl.obolibrary.org/obo/GAZ_00022402"/>
        <obo:IAO_0000115>A Local-Level Government Area of South Bougainville District.</obo:IAO_0000115>
        <oboInOwl:hasOBONamespace>GAZ</oboInOwl:hasOBONamespace>
        <oboInOwl:id>GAZ:00022407</oboInOwl:id>
        <rdfs:label>Torokina Rural Local-Level Government Area</rdfs:label>
    </owl:NamedIndividual>
    


    <!-- http://purl.obolibrary.org/obo/GAZ_00022408 -->

    <owl:NamedIndividual rdf:about="http://purl.obolibrary.org/obo/GAZ_00022408">
        <obo:RO_0001025 rdf:resource="http://purl.obolibrary.org/obo/GAZ_00022402"/>
        <obo:IAO_0000115>A Local-Level Government Area of South Bougainville District.</obo:IAO_0000115>
        <oboInOwl:hasOBONamespace>GAZ</oboInOwl:hasOBONamespace>
        <oboInOwl:id>GAZ:00022408</oboInOwl:id>
        <rdfs:label>Siwai Rural Local-Level Government Area</rdfs:label>
    </owl:NamedIndividual>
    


    <!-- http://purl.obolibrary.org/obo/GAZ_00022409 -->

    <owl:NamedIndividual rdf:about="http://purl.obolibrary.org/obo/GAZ_00022409">
        <rdf:type rdf:resource="http://purl.obolibrary.org/obo/ENVO_00000004"/>
        <obo:RO_0001025 rdf:resource="http://purl.obolibrary.org/obo/GAZ_00012662"/>
        <obo:IAO_0000115>A district of Northern Province, Papua New Guinea.</obo:IAO_0000115>
        <oboInOwl:hasOBONamespace>GAZ</oboInOwl:hasOBONamespace>
        <oboInOwl:id>GAZ:00022409</oboInOwl:id>
        <rdfs:label>Ijivitari District</rdfs:label>
    </owl:NamedIndividual>
    


    <!-- http://purl.obolibrary.org/obo/GAZ_00022410 -->

    <owl:NamedIndividual rdf:about="http://purl.obolibrary.org/obo/GAZ_00022410">
        <rdf:type rdf:resource="http://purl.obolibrary.org/obo/ENVO_00000004"/>
        <obo:RO_0001025 rdf:resource="http://purl.obolibrary.org/obo/GAZ_00012662"/>
        <obo:IAO_0000115>A district of Northern Province, Papua New Guinea.</obo:IAO_0000115>
        <oboInOwl:hasOBONamespace>GAZ</oboInOwl:hasOBONamespace>
        <oboInOwl:id>GAZ:00022410</oboInOwl:id>
        <rdfs:label>Sohe District</rdfs:label>
    </owl:NamedIndividual>
    


    <!-- http://purl.obolibrary.org/obo/GAZ_00022411 -->

    <owl:NamedIndividual rdf:about="http://purl.obolibrary.org/obo/GAZ_00022411">
        <obo:RO_0001025 rdf:resource="http://purl.obolibrary.org/obo/GAZ_00012658"/>
        <oboInOwl:hasOBONamespace>GAZ</oboInOwl:hasOBONamespace>
        <oboInOwl:id>GAZ:00022411</oboInOwl:id>
        <rdfs:label>Sina Sina-Yonggomugl District</rdfs:label>
    </owl:NamedIndividual>
    


    <!-- http://purl.obolibrary.org/obo/GAZ_00022412 -->

    <owl:NamedIndividual rdf:about="http://purl.obolibrary.org/obo/GAZ_00022412">
        <obo:RO_0001025 rdf:resource="http://purl.obolibrary.org/obo/GAZ_00012658"/>
        <oboInOwl:hasOBONamespace>GAZ</oboInOwl:hasOBONamespace>
        <oboInOwl:id>GAZ:00022412</oboInOwl:id>
        <rdfs:label>Karimui-Nomane District</rdfs:label>
    </owl:NamedIndividual>
    


    <!-- http://purl.obolibrary.org/obo/GAZ_00022413 -->

    <owl:NamedIndividual rdf:about="http://purl.obolibrary.org/obo/GAZ_00022413">
        <obo:RO_0001025 rdf:resource="http://purl.obolibrary.org/obo/GAZ_00012658"/>
        <oboInOwl:hasOBONamespace>GAZ</oboInOwl:hasOBONamespace>
        <oboInOwl:id>GAZ:00022413</oboInOwl:id>
        <rdfs:label>Chauve District</rdfs:label>
    </owl:NamedIndividual>
    


    <!-- http://purl.obolibrary.org/obo/GAZ_00022414 -->

    <owl:NamedIndividual rdf:about="http://purl.obolibrary.org/obo/GAZ_00022414">
        <obo:RO_0001025 rdf:resource="http://purl.obolibrary.org/obo/GAZ_00012658"/>
        <oboInOwl:hasOBONamespace>GAZ</oboInOwl:hasOBONamespace>
        <oboInOwl:id>GAZ:00022414</oboInOwl:id>
        <rdfs:label>Kerowagi District</rdfs:label>
    </owl:NamedIndividual>
    


    <!-- http://purl.obolibrary.org/obo/GAZ_00022415 -->

    <owl:NamedIndividual rdf:about="http://purl.obolibrary.org/obo/GAZ_00022415">
        <obo:RO_0001025 rdf:resource="http://purl.obolibrary.org/obo/GAZ_00012658"/>
        <oboInOwl:hasOBONamespace>GAZ</oboInOwl:hasOBONamespace>
        <oboInOwl:id>GAZ:00022415</oboInOwl:id>
        <rdfs:label>Kundiawa-Gembogl District</rdfs:label>
    </owl:NamedIndividual>
    


    <!-- http://purl.obolibrary.org/obo/GAZ_00022416 -->

    <owl:NamedIndividual rdf:about="http://purl.obolibrary.org/obo/GAZ_00022416">
        <obo:RO_0001025 rdf:resource="http://purl.obolibrary.org/obo/GAZ_00012658"/>
        <oboInOwl:hasOBONamespace>GAZ</oboInOwl:hasOBONamespace>
        <oboInOwl:id>GAZ:00022416</oboInOwl:id>
        <rdfs:label>Gumine District</rdfs:label>
    </owl:NamedIndividual>
    


    <!-- http://purl.obolibrary.org/obo/GAZ_00022417 -->

    <owl:NamedIndividual rdf:about="http://purl.obolibrary.org/obo/GAZ_00022417">
        <rdf:type rdf:resource="http://purl.obolibrary.org/obo/ENVO_00000004"/>
        <obo:RO_0001025 rdf:resource="http://purl.obolibrary.org/obo/GAZ_00012665"/>
        <obo:IAO_0000115>A district of Western Province, Papua New Guinea.</obo:IAO_0000115>
        <oboInOwl:hasOBONamespace>GAZ</oboInOwl:hasOBONamespace>
        <oboInOwl:id>GAZ:00022417</oboInOwl:id>
        <rdfs:label>North Fly District</rdfs:label>
    </owl:NamedIndividual>
    


    <!-- http://purl.obolibrary.org/obo/GAZ_00022418 -->

    <owl:NamedIndividual rdf:about="http://purl.obolibrary.org/obo/GAZ_00022418">
        <rdf:type rdf:resource="http://purl.obolibrary.org/obo/ENVO_00000004"/>
        <obo:RO_0001025 rdf:resource="http://purl.obolibrary.org/obo/GAZ_00012665"/>
        <obo:IAO_0000115>A district of Western Province, Papua New Guinea.</obo:IAO_0000115>
        <oboInOwl:hasOBONamespace>GAZ</oboInOwl:hasOBONamespace>
        <oboInOwl:id>GAZ:00022418</oboInOwl:id>
        <rdfs:label>South Fly District</rdfs:label>
    </owl:NamedIndividual>
    


    <!-- http://purl.obolibrary.org/obo/GAZ_00022419 -->

    <owl:NamedIndividual rdf:about="http://purl.obolibrary.org/obo/GAZ_00022419">
        <rdf:type rdf:resource="http://purl.obolibrary.org/obo/ENVO_00000004"/>
        <obo:RO_0001025 rdf:resource="http://purl.obolibrary.org/obo/GAZ_00012665"/>
        <obo:IAO_0000115>A district of Western Province, Papua New Guinea. The district covers the central area of the Western Province. It shares a Provincial border with Southern Highlands Province and Gulf Province in the east. It shares an international boundary with the Papua province of Indonesia in the west and borders South Fly District in the south, and the North Fly District in the north.</obo:IAO_0000115>
        <oboInOwl:hasOBONamespace>GAZ</oboInOwl:hasOBONamespace>
        <oboInOwl:id>GAZ:00022419</oboInOwl:id>
        <rdfs:label>Middle Fly District</rdfs:label>
    </owl:NamedIndividual>
    


    <!-- http://purl.obolibrary.org/obo/GAZ_00022420 -->

    <owl:NamedIndividual rdf:about="http://purl.obolibrary.org/obo/GAZ_00022420">
        <rdf:type rdf:resource="http://purl.obolibrary.org/obo/ENVO_00000004"/>
        <obo:RO_0001025 rdf:resource="http://purl.obolibrary.org/obo/GAZ_00012661"/>
        <obo:IAO_0000115>A district of Western Highlands Province.</obo:IAO_0000115>
        <oboInOwl:hasOBONamespace>GAZ</oboInOwl:hasOBONamespace>
        <oboInOwl:id>GAZ:00022420</oboInOwl:id>
        <rdfs:label>Dei District</rdfs:label>
    </owl:NamedIndividual>
    


    <!-- http://purl.obolibrary.org/obo/GAZ_00022421 -->

    <owl:NamedIndividual rdf:about="http://purl.obolibrary.org/obo/GAZ_00022421">
        <rdf:type rdf:resource="http://purl.obolibrary.org/obo/ENVO_00000004"/>
        <obo:RO_0001025 rdf:resource="http://purl.obolibrary.org/obo/GAZ_00012661"/>
        <obo:IAO_0000115>A district of Western Highlands Province.</obo:IAO_0000115>
        <oboInOwl:hasOBONamespace>GAZ</oboInOwl:hasOBONamespace>
        <oboInOwl:id>GAZ:00022421</oboInOwl:id>
        <rdfs:label>Anglimp-South Waghi District</rdfs:label>
    </owl:NamedIndividual>
    


    <!-- http://purl.obolibrary.org/obo/GAZ_00022422 -->

    <owl:NamedIndividual rdf:about="http://purl.obolibrary.org/obo/GAZ_00022422">
        <rdf:type rdf:resource="http://purl.obolibrary.org/obo/ENVO_00000004"/>
        <obo:RO_0001025 rdf:resource="http://purl.obolibrary.org/obo/GAZ_00012661"/>
        <obo:IAO_0000115>A district of Western Highlands Province.</obo:IAO_0000115>
        <oboInOwl:hasOBONamespace>GAZ</oboInOwl:hasOBONamespace>
        <oboInOwl:id>GAZ:00022422</oboInOwl:id>
        <rdfs:label>Mul-Baiyer District</rdfs:label>
    </owl:NamedIndividual>
    


    <!-- http://purl.obolibrary.org/obo/GAZ_00022423 -->

    <owl:NamedIndividual rdf:about="http://purl.obolibrary.org/obo/GAZ_00022423">
        <rdf:type rdf:resource="http://purl.obolibrary.org/obo/ENVO_00000004"/>
        <obo:RO_0001025 rdf:resource="http://purl.obolibrary.org/obo/GAZ_00012661"/>
        <obo:IAO_0000115>A district of Western Highlands Province.</obo:IAO_0000115>
        <oboInOwl:hasOBONamespace>GAZ</oboInOwl:hasOBONamespace>
        <oboInOwl:id>GAZ:00022423</oboInOwl:id>
        <rdfs:label>Mount Hagen District</rdfs:label>
    </owl:NamedIndividual>
    


    <!-- http://purl.obolibrary.org/obo/GAZ_00022424 -->

    <owl:NamedIndividual rdf:about="http://purl.obolibrary.org/obo/GAZ_00022424">
        <rdf:type rdf:resource="http://purl.obolibrary.org/obo/ENVO_00000004"/>
        <obo:RO_0001025 rdf:resource="http://purl.obolibrary.org/obo/GAZ_00012661"/>
        <obo:IAO_0000115>A district of Western Highlands Province.</obo:IAO_0000115>
        <oboInOwl:hasOBONamespace>GAZ</oboInOwl:hasOBONamespace>
        <oboInOwl:id>GAZ:00022424</oboInOwl:id>
        <rdfs:label>Tambul-Nebilyer District</rdfs:label>
    </owl:NamedIndividual>
    


    <!-- http://purl.obolibrary.org/obo/GAZ_00022425 -->

    <owl:NamedIndividual rdf:about="http://purl.obolibrary.org/obo/GAZ_00022425">
        <rdf:type rdf:resource="http://purl.obolibrary.org/obo/ENVO_00000004"/>
        <obo:RO_0001025 rdf:resource="http://purl.obolibrary.org/obo/GAZ_00012661"/>
        <obo:IAO_0000115>A district of Western Highlands Province.</obo:IAO_0000115>
        <oboInOwl:hasOBONamespace>GAZ</oboInOwl:hasOBONamespace>
        <oboInOwl:id>GAZ:00022425</oboInOwl:id>
        <rdfs:label>Jimi District</rdfs:label>
    </owl:NamedIndividual>
    


    <!-- http://purl.obolibrary.org/obo/GAZ_00022426 -->

    <owl:NamedIndividual rdf:about="http://purl.obolibrary.org/obo/GAZ_00022426">
        <rdf:type rdf:resource="http://purl.obolibrary.org/obo/ENVO_00000004"/>
        <obo:RO_0001025 rdf:resource="http://purl.obolibrary.org/obo/GAZ_00012661"/>
        <obo:IAO_0000115>A district of Western Highlands Province.</obo:IAO_0000115>
        <oboInOwl:hasOBONamespace>GAZ</oboInOwl:hasOBONamespace>
        <oboInOwl:id>GAZ:00022426</oboInOwl:id>
        <rdfs:label>North Waghi District</rdfs:label>
    </owl:NamedIndividual>
    


    <!-- http://purl.obolibrary.org/obo/GAZ_00022427 -->

    <owl:NamedIndividual rdf:about="http://purl.obolibrary.org/obo/GAZ_00022427">
        <rdf:type rdf:resource="http://purl.obolibrary.org/obo/ENVO_00000004"/>
        <obo:RO_0001025 rdf:resource="http://purl.obolibrary.org/obo/GAZ_00005191"/>
        <obo:IAO_0000115>A district in West New Britain Province, Papua New Guinea.</obo:IAO_0000115>
        <oboInOwl:hasOBONamespace>GAZ</oboInOwl:hasOBONamespace>
        <oboInOwl:id>GAZ:00022427</oboInOwl:id>
        <rdfs:label>Talasea District</rdfs:label>
    </owl:NamedIndividual>
    


    <!-- http://purl.obolibrary.org/obo/GAZ_00022428 -->

    <owl:NamedIndividual rdf:about="http://purl.obolibrary.org/obo/GAZ_00022428">
        <rdf:type rdf:resource="http://purl.obolibrary.org/obo/ENVO_00000004"/>
        <obo:RO_0001025 rdf:resource="http://purl.obolibrary.org/obo/GAZ_00012664"/>
        <obo:IAO_0000115>A district of Southern Highlands Province, Papua New Guinea.</obo:IAO_0000115>
        <oboInOwl:hasOBONamespace>GAZ</oboInOwl:hasOBONamespace>
        <oboInOwl:id>GAZ:00022428</oboInOwl:id>
        <rdfs:label>Komo-Magarima District</rdfs:label>
    </owl:NamedIndividual>
    


    <!-- http://purl.obolibrary.org/obo/GAZ_00022429 -->

    <owl:NamedIndividual rdf:about="http://purl.obolibrary.org/obo/GAZ_00022429">
        <rdf:type rdf:resource="http://purl.obolibrary.org/obo/ENVO_00000004"/>
        <obo:RO_0001025 rdf:resource="http://purl.obolibrary.org/obo/GAZ_00005191"/>
        <obo:IAO_0000115>A district in West New Britain Province, Papua New Guinea.</obo:IAO_0000115>
        <oboInOwl:hasOBONamespace>GAZ</oboInOwl:hasOBONamespace>
        <oboInOwl:id>GAZ:00022429</oboInOwl:id>
        <rdfs:label>Kandrian-Gloucester District</rdfs:label>
    </owl:NamedIndividual>
    


    <!-- http://purl.obolibrary.org/obo/GAZ_00022430 -->

    <owl:NamedIndividual rdf:about="http://purl.obolibrary.org/obo/GAZ_00022430">
        <rdf:type rdf:resource="http://purl.obolibrary.org/obo/ENVO_00000004"/>
        <obo:RO_0001025 rdf:resource="http://purl.obolibrary.org/obo/GAZ_00012663"/>
        <obo:IAO_0000115>A district of Sandaun Province.</obo:IAO_0000115>
        <oboInOwl:hasOBONamespace>GAZ</oboInOwl:hasOBONamespace>
        <oboInOwl:id>GAZ:00022430</oboInOwl:id>
        <rdfs:label>Aitape-Lumi District</rdfs:label>
    </owl:NamedIndividual>
    


    <!-- http://purl.obolibrary.org/obo/GAZ_00022431 -->

    <owl:NamedIndividual rdf:about="http://purl.obolibrary.org/obo/GAZ_00022431">
        <rdf:type rdf:resource="http://purl.obolibrary.org/obo/ENVO_00000004"/>
        <obo:RO_0001025 rdf:resource="http://purl.obolibrary.org/obo/GAZ_00012663"/>
        <obo:IAO_0000115>A district of Sandaun Province.</obo:IAO_0000115>
        <oboInOwl:hasOBONamespace>GAZ</oboInOwl:hasOBONamespace>
        <oboInOwl:id>GAZ:00022431</oboInOwl:id>
        <rdfs:label>Nuku District</rdfs:label>
    </owl:NamedIndividual>
    


    <!-- http://purl.obolibrary.org/obo/GAZ_00022432 -->

    <owl:NamedIndividual rdf:about="http://purl.obolibrary.org/obo/GAZ_00022432">
        <rdf:type rdf:resource="http://purl.obolibrary.org/obo/ENVO_00000004"/>
        <obo:RO_0001025 rdf:resource="http://purl.obolibrary.org/obo/GAZ_00012663"/>
        <obo:IAO_0000115>A district of Sandaun Province.</obo:IAO_0000115>
        <oboInOwl:hasOBONamespace>GAZ</oboInOwl:hasOBONamespace>
        <oboInOwl:id>GAZ:00022432</oboInOwl:id>
        <rdfs:label>Vanimo-Green River District</rdfs:label>
    </owl:NamedIndividual>
    


    <!-- http://purl.obolibrary.org/obo/GAZ_00022433 -->

    <owl:NamedIndividual rdf:about="http://purl.obolibrary.org/obo/GAZ_00022433">
        <rdf:type rdf:resource="http://purl.obolibrary.org/obo/ENVO_00000004"/>
        <obo:RO_0001025 rdf:resource="http://purl.obolibrary.org/obo/GAZ_00012663"/>
        <obo:IAO_0000115>A district of Sandaun Province.</obo:IAO_0000115>
        <oboInOwl:hasOBONamespace>GAZ</oboInOwl:hasOBONamespace>
        <oboInOwl:id>GAZ:00022433</oboInOwl:id>
        <rdfs:label>Telefomin District</rdfs:label>
    </owl:NamedIndividual>
    


    <!-- http://purl.obolibrary.org/obo/GAZ_00022434 -->

    <owl:NamedIndividual rdf:about="http://purl.obolibrary.org/obo/GAZ_00022434">
        <rdf:type rdf:resource="http://purl.obolibrary.org/obo/ENVO_00000004"/>
        <obo:RO_0001025 rdf:resource="http://purl.obolibrary.org/obo/GAZ_00012664"/>
        <obo:IAO_0000115>A district of Southern Highlands Province, Papua New Guinea.</obo:IAO_0000115>
        <oboInOwl:hasOBONamespace>GAZ</oboInOwl:hasOBONamespace>
        <oboInOwl:id>GAZ:00022434</oboInOwl:id>
        <rdfs:label>Nipa-Kutubu District</rdfs:label>
    </owl:NamedIndividual>
    


    <!-- http://purl.obolibrary.org/obo/GAZ_00022435 -->

    <owl:NamedIndividual rdf:about="http://purl.obolibrary.org/obo/GAZ_00022435">
        <rdf:type rdf:resource="http://purl.obolibrary.org/obo/ENVO_00000004"/>
        <obo:RO_0001025 rdf:resource="http://purl.obolibrary.org/obo/GAZ_00012664"/>
        <obo:IAO_0000115>A district of Southern Highlands Province, Papua New Guinea.</obo:IAO_0000115>
        <oboInOwl:hasOBONamespace>GAZ</oboInOwl:hasOBONamespace>
        <oboInOwl:id>GAZ:00022435</oboInOwl:id>
        <rdfs:label>Tari-Pori District</rdfs:label>
    </owl:NamedIndividual>
    


    <!-- http://purl.obolibrary.org/obo/GAZ_00022436 -->

    <owl:NamedIndividual rdf:about="http://purl.obolibrary.org/obo/GAZ_00022436">
        <rdf:type rdf:resource="http://purl.obolibrary.org/obo/ENVO_00000004"/>
        <obo:RO_0001025 rdf:resource="http://purl.obolibrary.org/obo/GAZ_00012664"/>
        <obo:IAO_0000115>A district of Southern Highlands Province, Papua New Guinea.</obo:IAO_0000115>
        <oboInOwl:hasOBONamespace>GAZ</oboInOwl:hasOBONamespace>
        <oboInOwl:id>GAZ:00022436</oboInOwl:id>
        <rdfs:label>Imbonggu District</rdfs:label>
    </owl:NamedIndividual>
    


    <!-- http://purl.obolibrary.org/obo/GAZ_00022437 -->

    <owl:NamedIndividual rdf:about="http://purl.obolibrary.org/obo/GAZ_00022437">
        <rdf:type rdf:resource="http://purl.obolibrary.org/obo/ENVO_00000004"/>
        <obo:RO_0001025 rdf:resource="http://purl.obolibrary.org/obo/GAZ_00012664"/>
        <obo:IAO_0000115>A district of Southern Highlands Province, Papua New Guinea.</obo:IAO_0000115>
        <oboInOwl:hasOBONamespace>GAZ</oboInOwl:hasOBONamespace>
        <oboInOwl:id>GAZ:00022437</oboInOwl:id>
        <rdfs:label>Ialibu-Pangia District</rdfs:label>
    </owl:NamedIndividual>
    


    <!-- http://purl.obolibrary.org/obo/GAZ_00022438 -->

    <owl:NamedIndividual rdf:about="http://purl.obolibrary.org/obo/GAZ_00022438">
        <rdf:type rdf:resource="http://purl.obolibrary.org/obo/ENVO_00000004"/>
        <obo:RO_0001025 rdf:resource="http://purl.obolibrary.org/obo/GAZ_00012664"/>
        <obo:IAO_0000115>A district of Southern Highlands Province, Papua New Guinea.</obo:IAO_0000115>
        <oboInOwl:hasOBONamespace>GAZ</oboInOwl:hasOBONamespace>
        <oboInOwl:id>GAZ:00022438</oboInOwl:id>
        <rdfs:label>Kagua-Erave District</rdfs:label>
    </owl:NamedIndividual>
    


    <!-- http://purl.obolibrary.org/obo/GAZ_00022439 -->

    <owl:NamedIndividual rdf:about="http://purl.obolibrary.org/obo/GAZ_00022439">
        <rdf:type rdf:resource="http://purl.obolibrary.org/obo/ENVO_00000004"/>
        <obo:RO_0001025 rdf:resource="http://purl.obolibrary.org/obo/GAZ_00012664"/>
        <obo:IAO_0000115>A district of Southern Highlands Province, Papua New Guinea.</obo:IAO_0000115>
        <oboInOwl:hasOBONamespace>GAZ</oboInOwl:hasOBONamespace>
        <oboInOwl:id>GAZ:00022439</oboInOwl:id>
        <rdfs:label>Mendi-Munihu District</rdfs:label>
    </owl:NamedIndividual>
    


    <!-- http://purl.obolibrary.org/obo/GAZ_00022440 -->

    <owl:NamedIndividual rdf:about="http://purl.obolibrary.org/obo/GAZ_00022440">
        <rdf:type rdf:resource="http://purl.obolibrary.org/obo/ENVO_00000004"/>
        <obo:RO_0001025 rdf:resource="http://purl.obolibrary.org/obo/GAZ_00012664"/>
        <obo:IAO_0000115>A district of Southern Highlands Province, Papua New Guinea.</obo:IAO_0000115>
        <oboInOwl:hasOBONamespace>GAZ</oboInOwl:hasOBONamespace>
        <oboInOwl:id>GAZ:00022440</oboInOwl:id>
        <rdfs:label>Koroba-Kopiago District</rdfs:label>
    </owl:NamedIndividual>
    


    <!-- http://purl.obolibrary.org/obo/GAZ_00051283 -->

    <owl:NamedIndividual rdf:about="http://purl.obolibrary.org/obo/GAZ_00051283">
        <rdf:type rdf:resource="http://purl.obolibrary.org/obo/ENVO_00000222"/>
        <obo:RO_0001025 rdf:resource="http://purl.obolibrary.org/obo/GAZ_00005193"/>
        <obo:IAO_0000115>A volcanic island between the mainland of Papua New Guinea and the island of New Britain. It is separated from New Britain by Dampier Strait. It is comprised of several coalescing stratovolcanoes that are cut by a large 13 x 17 km caldera whose walls rise up to 1 km above its floor. The caldera is widely breached to the sea on the NE side and contains three youthful post-caldera cones with summit crater lakes, Talo, Soal, and Barik. The largest of these cones, 1494 m high Talo, displays several thermal areas and has satellitic cones on its flanks.</obo:IAO_0000115>
        <oboInOwl:hasOBONamespace>GAZ</oboInOwl:hasOBONamespace>
        <oboInOwl:id>GAZ:00051283</oboInOwl:id>
        <rdfs:label>Umboi Island</rdfs:label>
    </owl:NamedIndividual>
    


    <!-- http://purl.obolibrary.org/obo/GAZ_00051285 -->

    <owl:NamedIndividual rdf:about="http://purl.obolibrary.org/obo/GAZ_00051285">
        <obo:RO_0001025 rdf:resource="http://purl.obolibrary.org/obo/GAZ_00005193"/>
        <obo:IAO_0000115>A volcanic island northwest of New Britain in the Bismarck Sea. An incised stratovolcano with a summit crater lake. Deep valleys cut the flanks of the volcano, which is partially surrounded by coral reefs. An older volcano that forms much of the island consists mainly of porphyritic basaltic rocks. A younger andesitic cone with a 1.5 km wide crater has been constructed within the older volcano&apos;s larger crater, whose rim is exposed on the northern and eastern sides.</obo:IAO_0000115>
        <oboInOwl:hasOBONamespace>GAZ</oboInOwl:hasOBONamespace>
        <oboInOwl:id>GAZ:00051285</oboInOwl:id>
        <rdfs:label>Sakar Island</rdfs:label>
    </owl:NamedIndividual>
    


    <!-- http://purl.obolibrary.org/obo/GAZ_00051589 -->

    <owl:NamedIndividual rdf:about="http://purl.obolibrary.org/obo/GAZ_00051589">
        <obo:RO_0001025 rdf:resource="http://purl.obolibrary.org/obo/GAZ_00012666"/>
        <obo:RO_0001025 rdf:resource="http://purl.obolibrary.org/obo/GAZ_00051599"/>
        <obo:IAO_0000115>A group of islands in Milne Bay and considered part of Papua New Guinea. They consist of Dugumenu, Gawa, Iwa Island and Kwaiawata. They are usually considered to be part of the Woodlark Islands group.</obo:IAO_0000115>
        <oboInOwl:hasOBONamespace>GAZ</oboInOwl:hasOBONamespace>
        <oboInOwl:id>GAZ:00051589</oboInOwl:id>
        <rdfs:label>Marshall Bennett Islands</rdfs:label>
    </owl:NamedIndividual>
    


    <!-- http://purl.obolibrary.org/obo/GAZ_00051590 -->

    <owl:NamedIndividual rdf:about="http://purl.obolibrary.org/obo/GAZ_00051590">
        <obo:RO_0001025 rdf:resource="http://purl.obolibrary.org/obo/GAZ_00022379"/>
        <obo:RO_0001025 rdf:resource="http://purl.obolibrary.org/obo/GAZ_00051599"/>
        <obo:IAO_0000115>An island in Milne Bay Province, Papua New Guinea.</obo:IAO_0000115>
        <oboInOwl:hasOBONamespace>GAZ</oboInOwl:hasOBONamespace>
        <oboInOwl:id>GAZ:00051590</oboInOwl:id>
        <rdfs:label>Woodlark Island</rdfs:label>
    </owl:NamedIndividual>
    


    <!-- http://purl.obolibrary.org/obo/GAZ_00051591 -->

    <owl:NamedIndividual rdf:about="http://purl.obolibrary.org/obo/GAZ_00051591">
        <obo:RO_0001025 rdf:resource="http://purl.obolibrary.org/obo/GAZ_00051589"/>
        <obo:IAO_0000115>One of the Marshall Bennett Islands.</obo:IAO_0000115>
        <oboInOwl:hasOBONamespace>GAZ</oboInOwl:hasOBONamespace>
        <oboInOwl:id>GAZ:00051591</oboInOwl:id>
        <rdfs:label>Dugumenu Island</rdfs:label>
    </owl:NamedIndividual>
    


    <!-- http://purl.obolibrary.org/obo/GAZ_00051592 -->

    <owl:NamedIndividual rdf:about="http://purl.obolibrary.org/obo/GAZ_00051592">
        <obo:RO_0001025 rdf:resource="http://purl.obolibrary.org/obo/GAZ_00051589"/>
        <obo:IAO_0000115>One of the Marshall Bennett Islands.</obo:IAO_0000115>
        <oboInOwl:hasOBONamespace>GAZ</oboInOwl:hasOBONamespace>
        <oboInOwl:id>GAZ:00051592</oboInOwl:id>
        <rdfs:label>Gawa Island</rdfs:label>
    </owl:NamedIndividual>
    


    <!-- http://purl.obolibrary.org/obo/GAZ_00051593 -->

    <owl:NamedIndividual rdf:about="http://purl.obolibrary.org/obo/GAZ_00051593">
        <obo:RO_0001025 rdf:resource="http://purl.obolibrary.org/obo/GAZ_00051589"/>
        <obo:IAO_0000115>One of the Marshall Bennett Islands.</obo:IAO_0000115>
        <oboInOwl:hasOBONamespace>GAZ</oboInOwl:hasOBONamespace>
        <oboInOwl:id>GAZ:00051593</oboInOwl:id>
        <rdfs:label>Kwaiawata Island</rdfs:label>
    </owl:NamedIndividual>
    


    <!-- http://purl.obolibrary.org/obo/GAZ_00051594 -->

    <owl:NamedIndividual rdf:about="http://purl.obolibrary.org/obo/GAZ_00051594">
        <obo:RO_0001025 rdf:resource="http://purl.obolibrary.org/obo/GAZ_00051589"/>
        <obo:IAO_0000115>One of the Marshall Bennett Islands.</obo:IAO_0000115>
        <oboInOwl:hasOBONamespace>GAZ</oboInOwl:hasOBONamespace>
        <oboInOwl:id>GAZ:00051594</oboInOwl:id>
        <rdfs:label>Iwa Island</rdfs:label>
    </owl:NamedIndividual>
    


    <!-- http://purl.obolibrary.org/obo/GAZ_00051595 -->

    <owl:NamedIndividual rdf:about="http://purl.obolibrary.org/obo/GAZ_00051595">
        <rdf:type rdf:resource="http://purl.obolibrary.org/obo/ENVO_00000220"/>
        <obo:RO_0001025 rdf:resource="http://purl.obolibrary.org/obo/GAZ_00007181"/>
        <obo:IAO_0000115>An island group within the D&apos;Entrecasteaux Islands.</obo:IAO_0000115>
        <oboInOwl:hasOBONamespace>GAZ</oboInOwl:hasOBONamespace>
        <oboInOwl:id>GAZ:00051595</oboInOwl:id>
        <rdfs:label>Amphlett Islands</rdfs:label>
    </owl:NamedIndividual>
    


    <!-- http://purl.obolibrary.org/obo/GAZ_00051596 -->

    <owl:NamedIndividual rdf:about="http://purl.obolibrary.org/obo/GAZ_00051596">
        <obo:RO_0001025 rdf:resource="http://purl.obolibrary.org/obo/GAZ_00022379"/>
        <obo:RO_0001025 rdf:resource="http://purl.obolibrary.org/obo/GAZ_00051599"/>
        <obo:IAO_0000115>An island in Milne Bay Province, Papua New Guinea. Located off the south-eastern tip of New Guinea in the China Strait Samarai has an area of just 240,000 m2.</obo:IAO_0000115>
        <oboInOwl:hasOBONamespace>GAZ</oboInOwl:hasOBONamespace>
        <oboInOwl:id>GAZ:00051596</oboInOwl:id>
        <rdfs:label>Samarai Island</rdfs:label>
    </owl:NamedIndividual>
    


    <!-- http://purl.obolibrary.org/obo/GAZ_00051597 -->

    <owl:NamedIndividual rdf:about="http://purl.obolibrary.org/obo/GAZ_00051597">
        <obo:RO_0001025 rdf:resource="http://purl.obolibrary.org/obo/GAZ_00022379"/>
        <obo:RO_0001025 rdf:resource="http://purl.obolibrary.org/obo/GAZ_00051599"/>
        <oboInOwl:hasOBONamespace>GAZ</oboInOwl:hasOBONamespace>
        <oboInOwl:id>GAZ:00051597</oboInOwl:id>
        <rdfs:label>Engineer Islands</rdfs:label>
    </owl:NamedIndividual>
    


    <!-- http://purl.obolibrary.org/obo/GAZ_00051598 -->

    <owl:NamedIndividual rdf:about="http://purl.obolibrary.org/obo/GAZ_00051598">
        <obo:RO_0001025 rdf:resource="http://purl.obolibrary.org/obo/GAZ_00012666"/>
        <obo:RO_0001025 rdf:resource="http://purl.obolibrary.org/obo/GAZ_00051599"/>
        <oboInOwl:hasOBONamespace>GAZ</oboInOwl:hasOBONamespace>
        <oboInOwl:id>GAZ:00051598</oboInOwl:id>
        <rdfs:label>Deka Deka Islands</rdfs:label>
    </owl:NamedIndividual>
    


    <!-- http://purl.obolibrary.org/obo/GAZ_00051599 -->

    <owl:NamedIndividual rdf:about="http://purl.obolibrary.org/obo/GAZ_00051599">
        <obo:RO_0001025 rdf:resource="http://purl.obolibrary.org/obo/GAZ_00012666"/>
        <obo:IAO_0000115>A large bay in Milne Bay Province, southeastern Papua New Guinea.</obo:IAO_0000115>
        <oboInOwl:hasOBONamespace>GAZ</oboInOwl:hasOBONamespace>
        <oboInOwl:id>GAZ:00051599</oboInOwl:id>
        <rdfs:label>Milne Bay</rdfs:label>
    </owl:NamedIndividual>
    


    <!-- http://purl.obolibrary.org/obo/GAZ_00051600 -->

    <owl:NamedIndividual rdf:about="http://purl.obolibrary.org/obo/GAZ_00051600">
        <obo:RO_0001025 rdf:resource="http://purl.obolibrary.org/obo/GAZ_00012666"/>
        <obo:RO_0001025 rdf:resource="http://purl.obolibrary.org/obo/GAZ_00051599"/>
        <oboInOwl:hasOBONamespace>GAZ</oboInOwl:hasOBONamespace>
        <oboInOwl:id>GAZ:00051600</oboInOwl:id>
        <rdfs:label>Saliba Island</rdfs:label>
    </owl:NamedIndividual>
    


    <!-- http://purl.obolibrary.org/obo/GAZ_00051602 -->

    <owl:NamedIndividual rdf:about="http://purl.obolibrary.org/obo/GAZ_00051602">
        <obo:RO_0001025 rdf:resource="http://purl.obolibrary.org/obo/GAZ_00012666"/>
        <obo:RO_0001025 rdf:resource="http://purl.obolibrary.org/obo/GAZ_00051599"/>
        <oboInOwl:hasOBONamespace>GAZ</oboInOwl:hasOBONamespace>
        <oboInOwl:id>GAZ:00051602</oboInOwl:id>
        <rdfs:label>Logea Island</rdfs:label>
    </owl:NamedIndividual>
    


    <!-- http://purl.obolibrary.org/obo/GAZ_00051603 -->

    <owl:NamedIndividual rdf:about="http://purl.obolibrary.org/obo/GAZ_00051603">
        <obo:RO_0001025 rdf:resource="http://purl.obolibrary.org/obo/GAZ_00012666"/>
        <obo:RO_0001025 rdf:resource="http://purl.obolibrary.org/obo/GAZ_00051599"/>
        <oboInOwl:hasOBONamespace>GAZ</oboInOwl:hasOBONamespace>
        <oboInOwl:id>GAZ:00051603</oboInOwl:id>
        <rdfs:label>Kwato Island</rdfs:label>
    </owl:NamedIndividual>
    


    <!-- http://purl.obolibrary.org/obo/GAZ_00051637 -->

    <owl:NamedIndividual rdf:about="http://purl.obolibrary.org/obo/GAZ_00051637">
        <obo:RO_0001025 rdf:resource="http://purl.obolibrary.org/obo/GAZ_00007179"/>
        <obo:IAO_0000115>One of the Admiralty Islands.</obo:IAO_0000115>
        <oboInOwl:hasOBONamespace>GAZ</oboInOwl:hasOBONamespace>
        <oboInOwl:id>GAZ:00051637</oboInOwl:id>
        <rdfs:label>Ponam Island</rdfs:label>
    </owl:NamedIndividual>
    


    <!-- http://purl.obolibrary.org/obo/GAZ_00051638 -->

    <owl:NamedIndividual rdf:about="http://purl.obolibrary.org/obo/GAZ_00051638">
        <obo:RO_0001025 rdf:resource="http://purl.obolibrary.org/obo/GAZ_00007179"/>
        <obo:IAO_0000115>One of the Admiralty Islands.</obo:IAO_0000115>
        <oboInOwl:hasOBONamespace>GAZ</oboInOwl:hasOBONamespace>
        <oboInOwl:id>GAZ:00051638</oboInOwl:id>
        <rdfs:label>Noru Island</rdfs:label>
    </owl:NamedIndividual>
    


    <!-- http://purl.obolibrary.org/obo/GAZ_00051639 -->

    <owl:NamedIndividual rdf:about="http://purl.obolibrary.org/obo/GAZ_00051639">
        <obo:RO_0001025 rdf:resource="http://purl.obolibrary.org/obo/GAZ_00007179"/>
        <obo:IAO_0000115>One of the Admiralty islands.</obo:IAO_0000115>
        <oboInOwl:hasOBONamespace>GAZ</oboInOwl:hasOBONamespace>
        <oboInOwl:id>GAZ:00051639</oboInOwl:id>
        <rdfs:label>Sisi Island</rdfs:label>
    </owl:NamedIndividual>
    


    <!-- http://purl.obolibrary.org/obo/GAZ_00051640 -->

    <owl:NamedIndividual rdf:about="http://purl.obolibrary.org/obo/GAZ_00051640">
        <obo:RO_0001025 rdf:resource="http://purl.obolibrary.org/obo/GAZ_00007179"/>
        <obo:IAO_0000115>One of the Admiralty Islands.</obo:IAO_0000115>
        <oboInOwl:hasOBONamespace>GAZ</oboInOwl:hasOBONamespace>
        <oboInOwl:id>GAZ:00051640</oboInOwl:id>
        <rdfs:label>Pahi Island</rdfs:label>
    </owl:NamedIndividual>
    


    <!-- http://purl.obolibrary.org/obo/GAZ_00051641 -->

    <owl:NamedIndividual rdf:about="http://purl.obolibrary.org/obo/GAZ_00051641">
        <obo:RO_0001025 rdf:resource="http://purl.obolibrary.org/obo/GAZ_00007179"/>
        <obo:IAO_0000115>One of the Admiralty Islands.</obo:IAO_0000115>
        <oboInOwl:hasOBONamespace>GAZ</oboInOwl:hasOBONamespace>
        <oboInOwl:id>GAZ:00051641</oboInOwl:id>
        <rdfs:label>Pityilu Island</rdfs:label>
    </owl:NamedIndividual>
    


    <!-- http://purl.obolibrary.org/obo/GAZ_00051642 -->

    <owl:NamedIndividual rdf:about="http://purl.obolibrary.org/obo/GAZ_00051642">
        <obo:RO_0001025 rdf:resource="http://purl.obolibrary.org/obo/GAZ_00007179"/>
        <obo:IAO_0000115>One of the Admiralty Islands.</obo:IAO_0000115>
        <oboInOwl:hasOBONamespace>GAZ</oboInOwl:hasOBONamespace>
        <oboInOwl:id>GAZ:00051642</oboInOwl:id>
        <rdfs:label>Bundro Island</rdfs:label>
    </owl:NamedIndividual>
    


    <!-- http://purl.obolibrary.org/obo/GAZ_00051646 -->

    <owl:NamedIndividual rdf:about="http://purl.obolibrary.org/obo/GAZ_00051646">
        <obo:RO_0001025 rdf:resource="http://purl.obolibrary.org/obo/GAZ_00016822"/>
        <obo:RO_0001025 rdf:resource="http://purl.obolibrary.org/obo/GAZ_00022378"/>
        <obo:IAO_0000115>A low coral island of volcanic origin with a maximum elevation of 3 m above sea level. It is approximately 19.3 km in circumference and 4 km by 7.2 km in diameter with a surface area of 1,400 ha.</obo:IAO_0000115>
        <oboInOwl:hasOBONamespace>GAZ</oboInOwl:hasOBONamespace>
        <oboInOwl:id>GAZ:00051646</oboInOwl:id>
        <rdfs:label>Wuvulu Island</rdfs:label>
    </owl:NamedIndividual>
    


    <!-- http://purl.obolibrary.org/obo/GAZ_00051647 -->

    <owl:NamedIndividual rdf:about="http://purl.obolibrary.org/obo/GAZ_00051647">
        <obo:RO_0001025 rdf:resource="http://purl.obolibrary.org/obo/GAZ_00016822"/>
        <obo:IAO_0000115>An island in the Bismarck Archipelago. It is part of the Western Islands, Papua New Guinea.</obo:IAO_0000115>
        <oboInOwl:hasOBONamespace>GAZ</oboInOwl:hasOBONamespace>
        <oboInOwl:id>GAZ:00051647</oboInOwl:id>
        <rdfs:label>Aua Island</rdfs:label>
    </owl:NamedIndividual>
    


    <!-- http://purl.obolibrary.org/obo/GAZ_00051648 -->

    <owl:NamedIndividual rdf:about="http://purl.obolibrary.org/obo/GAZ_00051648">
        <obo:RO_0001025 rdf:resource="http://purl.obolibrary.org/obo/GAZ_00051656"/>
        <oboInOwl:hasOBONamespace>GAZ</oboInOwl:hasOBONamespace>
        <oboInOwl:id>GAZ:00051648</oboInOwl:id>
        <rdfs:label>Manu Island</rdfs:label>
    </owl:NamedIndividual>
    


    <!-- http://purl.obolibrary.org/obo/GAZ_00051649 -->

    <owl:NamedIndividual rdf:about="http://purl.obolibrary.org/obo/GAZ_00051649">
        <obo:RO_0001025 rdf:resource="http://purl.obolibrary.org/obo/GAZ_00016822"/>
        <obo:IAO_0000115>A group of islands located in the Western Islands region, situated 73 km west-northwest of the Hermit Islands and 255 km northwest of Manus Island (the largest of the Admiralty Islands); the PNG mainland is located 260 km to the south.</obo:IAO_0000115>
        <oboInOwl:hasOBONamespace>GAZ</oboInOwl:hasOBONamespace>
        <oboInOwl:id>GAZ:00051649</oboInOwl:id>
        <rdfs:label>Ninigo Islands</rdfs:label>
    </owl:NamedIndividual>
    


    <!-- http://purl.obolibrary.org/obo/GAZ_00051650 -->

    <owl:NamedIndividual rdf:about="http://purl.obolibrary.org/obo/GAZ_00051650">
        <obo:RO_0001025 rdf:resource="http://purl.obolibrary.org/obo/GAZ_00051649"/>
        <obo:IAO_0000115>An atoll.</obo:IAO_0000115>
        <oboInOwl:hasOBONamespace>GAZ</oboInOwl:hasOBONamespace>
        <oboInOwl:id>GAZ:00051650</oboInOwl:id>
        <rdfs:label>Suymasuma Atoll</rdfs:label>
    </owl:NamedIndividual>
    


    <!-- http://purl.obolibrary.org/obo/GAZ_00051651 -->

    <owl:NamedIndividual rdf:about="http://purl.obolibrary.org/obo/GAZ_00051651">
        <obo:RO_0001025 rdf:resource="http://purl.obolibrary.org/obo/GAZ_00051649"/>
        <obo:IAO_0000115>An atoll.</obo:IAO_0000115>
        <oboInOwl:hasOBONamespace>GAZ</oboInOwl:hasOBONamespace>
        <oboInOwl:id>GAZ:00051651</oboInOwl:id>
        <rdfs:label>Sama Group</rdfs:label>
    </owl:NamedIndividual>
    


    <!-- http://purl.obolibrary.org/obo/GAZ_00051653 -->

    <owl:NamedIndividual rdf:about="http://purl.obolibrary.org/obo/GAZ_00051653">
        <obo:RO_0001025 rdf:resource="http://purl.obolibrary.org/obo/GAZ_00051649"/>
        <obo:IAO_0000115>An atoll.</obo:IAO_0000115>
        <oboInOwl:hasOBONamespace>GAZ</oboInOwl:hasOBONamespace>
        <oboInOwl:id>GAZ:00051653</oboInOwl:id>
        <rdfs:label>Awin Atoll</rdfs:label>
    </owl:NamedIndividual>
    


    <!-- http://purl.obolibrary.org/obo/GAZ_00051654 -->

    <owl:NamedIndividual rdf:about="http://purl.obolibrary.org/obo/GAZ_00051654">
        <obo:RO_0001025 rdf:resource="http://purl.obolibrary.org/obo/GAZ_00051649"/>
        <obo:IAO_0000115>An atoll located 5 km east of the Pelleluhu Group.</obo:IAO_0000115>
        <oboInOwl:hasOBONamespace>GAZ</oboInOwl:hasOBONamespace>
        <oboInOwl:id>GAZ:00051654</oboInOwl:id>
        <rdfs:label>Heina Group</rdfs:label>
    </owl:NamedIndividual>
    


    <!-- http://purl.obolibrary.org/obo/GAZ_00051655 -->

    <owl:NamedIndividual rdf:about="http://purl.obolibrary.org/obo/GAZ_00051655">
        <obo:RO_0001025 rdf:resource="http://purl.obolibrary.org/obo/GAZ_00051649"/>
        <obo:IAO_0000115>An atoll located 19 km east of Ninigo. Liot consists of a tiny central lagoon surrounded on three sides by the solitary island of Ufe; the western side is composed of submerged reef formations.</obo:IAO_0000115>
        <oboInOwl:hasOBONamespace>GAZ</oboInOwl:hasOBONamespace>
        <oboInOwl:id>GAZ:00051655</oboInOwl:id>
        <rdfs:label>Liot Atoll</rdfs:label>
    </owl:NamedIndividual>
    


    <!-- http://purl.obolibrary.org/obo/GAZ_00051656 -->

    <owl:NamedIndividual rdf:about="http://purl.obolibrary.org/obo/GAZ_00051656">
        <obo:RO_0001025 rdf:resource="http://purl.obolibrary.org/obo/GAZ_00051649"/>
        <obo:IAO_0000115>An atoll structure of 9 by 8 km consisting of a small central lagoon that is completely surrounded by comparatively broad reefs. Located a few hundred meters to the northeast from the Ninigo Group.</obo:IAO_0000115>
        <oboInOwl:hasOBONamespace>GAZ</oboInOwl:hasOBONamespace>
        <oboInOwl:id>GAZ:00051656</oboInOwl:id>
        <rdfs:label>Pelleluhu Group</rdfs:label>
    </owl:NamedIndividual>
    


    <!-- http://purl.obolibrary.org/obo/GAZ_00051657 -->

    <owl:NamedIndividual rdf:about="http://purl.obolibrary.org/obo/GAZ_00051657">
        <obo:RO_0001025 rdf:resource="http://purl.obolibrary.org/obo/GAZ_00051649"/>
        <oboInOwl:hasOBONamespace>GAZ</oboInOwl:hasOBONamespace>
        <oboInOwl:id>GAZ:00051657</oboInOwl:id>
        <rdfs:label>Pupol Reef</rdfs:label>
    </owl:NamedIndividual>
    


    <!-- http://purl.obolibrary.org/obo/GAZ_00051658 -->

    <owl:NamedIndividual rdf:about="http://purl.obolibrary.org/obo/GAZ_00051658">
        <obo:RO_0001025 rdf:resource="http://purl.obolibrary.org/obo/GAZ_00051651"/>
        <oboInOwl:hasOBONamespace>GAZ</oboInOwl:hasOBONamespace>
        <oboInOwl:id>GAZ:00051658</oboInOwl:id>
        <rdfs:label>Similam Island</rdfs:label>
    </owl:NamedIndividual>
    


    <!-- http://purl.obolibrary.org/obo/GAZ_00051659 -->

    <owl:NamedIndividual rdf:about="http://purl.obolibrary.org/obo/GAZ_00051659">
        <obo:RO_0001025 rdf:resource="http://purl.obolibrary.org/obo/GAZ_00051651"/>
        <oboInOwl:hasOBONamespace>GAZ</oboInOwl:hasOBONamespace>
        <oboInOwl:id>GAZ:00051659</oboInOwl:id>
        <rdfs:label>Sama Island</rdfs:label>
    </owl:NamedIndividual>
    


    <!-- http://purl.obolibrary.org/obo/GAZ_00051660 -->

    <owl:NamedIndividual rdf:about="http://purl.obolibrary.org/obo/GAZ_00051660">
        <obo:RO_0001025 rdf:resource="http://purl.obolibrary.org/obo/GAZ_00051651"/>
        <oboInOwl:hasOBONamespace>GAZ</oboInOwl:hasOBONamespace>
        <oboInOwl:id>GAZ:00051660</oboInOwl:id>
        <rdfs:label>Pataku Island</rdfs:label>
    </owl:NamedIndividual>
    


    <!-- http://purl.obolibrary.org/obo/GAZ_00051661 -->

    <owl:NamedIndividual rdf:about="http://purl.obolibrary.org/obo/GAZ_00051661">
        <obo:RO_0001025 rdf:resource="http://purl.obolibrary.org/obo/GAZ_00051675"/>
        <oboInOwl:hasOBONamespace>GAZ</oboInOwl:hasOBONamespace>
        <oboInOwl:id>GAZ:00051661</oboInOwl:id>
        <rdfs:label>Bahanat Island</rdfs:label>
    </owl:NamedIndividual>
    


    <!-- http://purl.obolibrary.org/obo/GAZ_00051662 -->

    <owl:NamedIndividual rdf:about="http://purl.obolibrary.org/obo/GAZ_00051662">
        <obo:RO_0001025 rdf:resource="http://purl.obolibrary.org/obo/GAZ_00051675"/>
        <oboInOwl:hasOBONamespace>GAZ</oboInOwl:hasOBONamespace>
        <oboInOwl:id>GAZ:00051662</oboInOwl:id>
        <rdfs:label>Pingilap Island</rdfs:label>
    </owl:NamedIndividual>
    


    <!-- http://purl.obolibrary.org/obo/GAZ_00051663 -->

    <owl:NamedIndividual rdf:about="http://purl.obolibrary.org/obo/GAZ_00051663">
        <obo:RO_0001025 rdf:resource="http://purl.obolibrary.org/obo/GAZ_00051673"/>
        <oboInOwl:hasOBONamespace>GAZ</oboInOwl:hasOBONamespace>
        <oboInOwl:id>GAZ:00051663</oboInOwl:id>
        <rdfs:label>Keholl island</rdfs:label>
    </owl:NamedIndividual>
    


    <!-- http://purl.obolibrary.org/obo/GAZ_00051664 -->

    <owl:NamedIndividual rdf:about="http://purl.obolibrary.org/obo/GAZ_00051664">
        <obo:RO_0001025 rdf:resource="http://purl.obolibrary.org/obo/GAZ_00051675"/>
        <oboInOwl:hasOBONamespace>GAZ</oboInOwl:hasOBONamespace>
        <oboInOwl:id>GAZ:00051664</oboInOwl:id>
        <rdfs:label>Hottom Island</rdfs:label>
    </owl:NamedIndividual>
    


    <!-- http://purl.obolibrary.org/obo/GAZ_00051665 -->

    <owl:NamedIndividual rdf:about="http://purl.obolibrary.org/obo/GAZ_00051665">
        <obo:RO_0001025 rdf:resource="http://purl.obolibrary.org/obo/GAZ_00051673"/>
        <oboInOwl:hasOBONamespace>GAZ</oboInOwl:hasOBONamespace>
        <oboInOwl:id>GAZ:00051665</oboInOwl:id>
        <rdfs:label>Sand Island</rdfs:label>
    </owl:NamedIndividual>
    


    <!-- http://purl.obolibrary.org/obo/GAZ_00051666 -->

    <owl:NamedIndividual rdf:about="http://purl.obolibrary.org/obo/GAZ_00051666">
        <obo:RO_0001025 rdf:resource="http://purl.obolibrary.org/obo/GAZ_00051675"/>
        <oboInOwl:hasOBONamespace>GAZ</oboInOwl:hasOBONamespace>
        <oboInOwl:id>GAZ:00051666</oboInOwl:id>
        <rdfs:label>Talil Island</rdfs:label>
    </owl:NamedIndividual>
    


    <!-- http://purl.obolibrary.org/obo/GAZ_00051667 -->

    <owl:NamedIndividual rdf:about="http://purl.obolibrary.org/obo/GAZ_00051667">
        <obo:RO_0001025 rdf:resource="http://purl.obolibrary.org/obo/GAZ_00051673"/>
        <oboInOwl:hasOBONamespace>GAZ</oboInOwl:hasOBONamespace>
        <oboInOwl:id>GAZ:00051667</oboInOwl:id>
        <rdfs:label>Nunu Island</rdfs:label>
    </owl:NamedIndividual>
    


    <!-- http://purl.obolibrary.org/obo/GAZ_00051668 -->

    <owl:NamedIndividual rdf:about="http://purl.obolibrary.org/obo/GAZ_00051668">
        <obo:RO_0001025 rdf:resource="http://purl.obolibrary.org/obo/GAZ_00051675"/>
        <oboInOwl:hasOBONamespace>GAZ</oboInOwl:hasOBONamespace>
        <oboInOwl:id>GAZ:00051668</oboInOwl:id>
        <rdfs:label>Amot Island</rdfs:label>
    </owl:NamedIndividual>
    


    <!-- http://purl.obolibrary.org/obo/GAZ_00051669 -->

    <owl:NamedIndividual rdf:about="http://purl.obolibrary.org/obo/GAZ_00051669">
        <obo:RO_0001025 rdf:resource="http://purl.obolibrary.org/obo/GAZ_00051673"/>
        <oboInOwl:hasOBONamespace>GAZ</oboInOwl:hasOBONamespace>
        <oboInOwl:id>GAZ:00051669</oboInOwl:id>
        <rdfs:label>Pisa Island</rdfs:label>
    </owl:NamedIndividual>
    


    <!-- http://purl.obolibrary.org/obo/GAZ_00051670 -->

    <owl:NamedIndividual rdf:about="http://purl.obolibrary.org/obo/GAZ_00051670">
        <obo:RO_0001025 rdf:resource="http://purl.obolibrary.org/obo/GAZ_00051673"/>
        <oboInOwl:hasOBONamespace>GAZ</oboInOwl:hasOBONamespace>
        <oboInOwl:id>GAZ:00051670</oboInOwl:id>
        <rdfs:label>Onia Island</rdfs:label>
    </owl:NamedIndividual>
    


    <!-- http://purl.obolibrary.org/obo/GAZ_00051671 -->

    <owl:NamedIndividual rdf:about="http://purl.obolibrary.org/obo/GAZ_00051671">
        <obo:RO_0001025 rdf:resource="http://purl.obolibrary.org/obo/GAZ_00051673"/>
        <oboInOwl:hasOBONamespace>GAZ</oboInOwl:hasOBONamespace>
        <oboInOwl:id>GAZ:00051671</oboInOwl:id>
        <rdfs:label>Sabucho Island</rdfs:label>
    </owl:NamedIndividual>
    


    <!-- http://purl.obolibrary.org/obo/GAZ_00051672 -->

    <owl:NamedIndividual rdf:about="http://purl.obolibrary.org/obo/GAZ_00051672">
        <obo:RO_0001025 rdf:resource="http://purl.obolibrary.org/obo/GAZ_00051673"/>
        <oboInOwl:hasOBONamespace>GAZ</oboInOwl:hasOBONamespace>
        <oboInOwl:id>GAZ:00051672</oboInOwl:id>
        <rdfs:label>Wahangahun Island</rdfs:label>
    </owl:NamedIndividual>
    


    <!-- http://purl.obolibrary.org/obo/GAZ_00051673 -->

    <owl:NamedIndividual rdf:about="http://purl.obolibrary.org/obo/GAZ_00051673">
        <obo:RO_0001025 rdf:resource="http://purl.obolibrary.org/obo/GAZ_00253928"/>
        <obo:IAO_0000115>An atoll.</obo:IAO_0000115>
        <oboInOwl:hasOBONamespace>GAZ</oboInOwl:hasOBONamespace>
        <oboInOwl:id>GAZ:00051673</oboInOwl:id>
        <rdfs:label>Ninigo Atoll</rdfs:label>
    </owl:NamedIndividual>
    


    <!-- http://purl.obolibrary.org/obo/GAZ_00051674 -->

    <owl:NamedIndividual rdf:about="http://purl.obolibrary.org/obo/GAZ_00051674">
        <obo:RO_0001025 rdf:resource="http://purl.obolibrary.org/obo/GAZ_00051673"/>
        <oboInOwl:hasOBONamespace>GAZ</oboInOwl:hasOBONamespace>
        <oboInOwl:id>GAZ:00051674</oboInOwl:id>
        <rdfs:label>Pihun Island</rdfs:label>
    </owl:NamedIndividual>
    


    <!-- http://purl.obolibrary.org/obo/GAZ_00051675 -->

    <owl:NamedIndividual rdf:about="http://purl.obolibrary.org/obo/GAZ_00051675">
        <obo:RO_0001025 rdf:resource="http://purl.obolibrary.org/obo/GAZ_00253928"/>
        <obo:IAO_0000115>The lagoon, open to the sea on its W side, of Ninigo Atoll.</obo:IAO_0000115>
        <oboInOwl:hasOBONamespace>GAZ</oboInOwl:hasOBONamespace>
        <oboInOwl:id>GAZ:00051675</oboInOwl:id>
        <rdfs:label>Ninigo Lagoon</rdfs:label>
    </owl:NamedIndividual>
    


    <!-- http://purl.obolibrary.org/obo/GAZ_00051676 -->

    <owl:NamedIndividual rdf:about="http://purl.obolibrary.org/obo/GAZ_00051676">
        <obo:RO_0001025 rdf:resource="http://purl.obolibrary.org/obo/GAZ_00051673"/>
        <oboInOwl:hasOBONamespace>GAZ</oboInOwl:hasOBONamespace>
        <oboInOwl:id>GAZ:00051676</oboInOwl:id>
        <rdfs:label>Kamochin Island</rdfs:label>
    </owl:NamedIndividual>
    


    <!-- http://purl.obolibrary.org/obo/GAZ_00051677 -->

    <owl:NamedIndividual rdf:about="http://purl.obolibrary.org/obo/GAZ_00051677">
        <obo:RO_0001025 rdf:resource="http://purl.obolibrary.org/obo/GAZ_00051673"/>
        <oboInOwl:hasOBONamespace>GAZ</oboInOwl:hasOBONamespace>
        <oboInOwl:id>GAZ:00051677</oboInOwl:id>
        <rdfs:label>Ngi Island</rdfs:label>
    </owl:NamedIndividual>
    


    <!-- http://purl.obolibrary.org/obo/GAZ_00051678 -->

    <owl:NamedIndividual rdf:about="http://purl.obolibrary.org/obo/GAZ_00051678">
        <obo:RO_0001025 rdf:resource="http://purl.obolibrary.org/obo/GAZ_00051673"/>
        <oboInOwl:hasOBONamespace>GAZ</oboInOwl:hasOBONamespace>
        <oboInOwl:id>GAZ:00051678</oboInOwl:id>
        <rdfs:label>Potaminam Island</rdfs:label>
    </owl:NamedIndividual>
    


    <!-- http://purl.obolibrary.org/obo/GAZ_00051679 -->

    <owl:NamedIndividual rdf:about="http://purl.obolibrary.org/obo/GAZ_00051679">
        <obo:RO_0001025 rdf:resource="http://purl.obolibrary.org/obo/GAZ_00051673"/>
        <oboInOwl:hasOBONamespace>GAZ</oboInOwl:hasOBONamespace>
        <oboInOwl:id>GAZ:00051679</oboInOwl:id>
        <rdfs:label>Amik Island</rdfs:label>
    </owl:NamedIndividual>
    


    <!-- http://purl.obolibrary.org/obo/GAZ_00051680 -->

    <owl:NamedIndividual rdf:about="http://purl.obolibrary.org/obo/GAZ_00051680">
        <obo:RO_0001025 rdf:resource="http://purl.obolibrary.org/obo/GAZ_00051673"/>
        <oboInOwl:hasOBONamespace>GAZ</oboInOwl:hasOBONamespace>
        <oboInOwl:id>GAZ:00051680</oboInOwl:id>
        <rdfs:label>Chacheon Island</rdfs:label>
    </owl:NamedIndividual>
    


    <!-- http://purl.obolibrary.org/obo/GAZ_00051681 -->

    <owl:NamedIndividual rdf:about="http://purl.obolibrary.org/obo/GAZ_00051681">
        <obo:RO_0001025 rdf:resource="http://purl.obolibrary.org/obo/GAZ_00051673"/>
        <oboInOwl:hasOBONamespace>GAZ</oboInOwl:hasOBONamespace>
        <oboInOwl:id>GAZ:00051681</oboInOwl:id>
        <rdfs:label>Maichuch Island</rdfs:label>
    </owl:NamedIndividual>
    


    <!-- http://purl.obolibrary.org/obo/GAZ_00051682 -->

    <owl:NamedIndividual rdf:about="http://purl.obolibrary.org/obo/GAZ_00051682">
        <obo:RO_0001025 rdf:resource="http://purl.obolibrary.org/obo/GAZ_00051673"/>
        <oboInOwl:hasOBONamespace>GAZ</oboInOwl:hasOBONamespace>
        <oboInOwl:id>GAZ:00051682</oboInOwl:id>
        <rdfs:label>Puol Island</rdfs:label>
    </owl:NamedIndividual>
    


    <!-- http://purl.obolibrary.org/obo/GAZ_00051683 -->

    <owl:NamedIndividual rdf:about="http://purl.obolibrary.org/obo/GAZ_00051683">
        <obo:RO_0001025 rdf:resource="http://purl.obolibrary.org/obo/GAZ_00051673"/>
        <oboInOwl:hasOBONamespace>GAZ</oboInOwl:hasOBONamespace>
        <oboInOwl:id>GAZ:00051683</oboInOwl:id>
        <rdfs:label>Chauch Island</rdfs:label>
    </owl:NamedIndividual>
    


    <!-- http://purl.obolibrary.org/obo/GAZ_00051684 -->

    <owl:NamedIndividual rdf:about="http://purl.obolibrary.org/obo/GAZ_00051684">
        <obo:RO_0001025 rdf:resource="http://purl.obolibrary.org/obo/GAZ_00051673"/>
        <oboInOwl:hasOBONamespace>GAZ</oboInOwl:hasOBONamespace>
        <oboInOwl:id>GAZ:00051684</oboInOwl:id>
        <rdfs:label>Hepisasa Island</rdfs:label>
    </owl:NamedIndividual>
    


    <!-- http://purl.obolibrary.org/obo/GAZ_00051685 -->

    <owl:NamedIndividual rdf:about="http://purl.obolibrary.org/obo/GAZ_00051685">
        <obo:RO_0001025 rdf:resource="http://purl.obolibrary.org/obo/GAZ_00051673"/>
        <oboInOwl:hasOBONamespace>GAZ</oboInOwl:hasOBONamespace>
        <oboInOwl:id>GAZ:00051685</oboInOwl:id>
        <rdfs:label>Ahu Island</rdfs:label>
    </owl:NamedIndividual>
    


    <!-- http://purl.obolibrary.org/obo/GAZ_00051686 -->

    <owl:NamedIndividual rdf:about="http://purl.obolibrary.org/obo/GAZ_00051686">
        <obo:RO_0001025 rdf:resource="http://purl.obolibrary.org/obo/GAZ_00051673"/>
        <oboInOwl:hasOBONamespace>GAZ</oboInOwl:hasOBONamespace>
        <oboInOwl:id>GAZ:00051686</oboInOwl:id>
        <rdfs:label>Hepi Island</rdfs:label>
    </owl:NamedIndividual>
    


    <!-- http://purl.obolibrary.org/obo/GAZ_00051687 -->

    <owl:NamedIndividual rdf:about="http://purl.obolibrary.org/obo/GAZ_00051687">
        <obo:RO_0001025 rdf:resource="http://purl.obolibrary.org/obo/GAZ_00051673"/>
        <oboInOwl:hasOBONamespace>GAZ</oboInOwl:hasOBONamespace>
        <oboInOwl:id>GAZ:00051687</oboInOwl:id>
        <rdfs:label>Mal Island</rdfs:label>
    </owl:NamedIndividual>
    


    <!-- http://purl.obolibrary.org/obo/GAZ_00051688 -->

    <owl:NamedIndividual rdf:about="http://purl.obolibrary.org/obo/GAZ_00051688">
        <obo:RO_0001025 rdf:resource="http://purl.obolibrary.org/obo/GAZ_00051673"/>
        <oboInOwl:hasOBONamespace>GAZ</oboInOwl:hasOBONamespace>
        <oboInOwl:id>GAZ:00051688</oboInOwl:id>
        <rdfs:label>Nahanu Island</rdfs:label>
    </owl:NamedIndividual>
    


    <!-- http://purl.obolibrary.org/obo/GAZ_00051689 -->

    <owl:NamedIndividual rdf:about="http://purl.obolibrary.org/obo/GAZ_00051689">
        <obo:RO_0001025 rdf:resource="http://purl.obolibrary.org/obo/GAZ_00051673"/>
        <oboInOwl:hasOBONamespace>GAZ</oboInOwl:hasOBONamespace>
        <oboInOwl:id>GAZ:00051689</oboInOwl:id>
        <rdfs:label>Longan Island</rdfs:label>
    </owl:NamedIndividual>
    


    <!-- http://purl.obolibrary.org/obo/GAZ_00051690 -->

    <owl:NamedIndividual rdf:about="http://purl.obolibrary.org/obo/GAZ_00051690">
        <obo:RO_0001025 rdf:resource="http://purl.obolibrary.org/obo/GAZ_00051673"/>
        <oboInOwl:hasOBONamespace>GAZ</oboInOwl:hasOBONamespace>
        <oboInOwl:id>GAZ:00051690</oboInOwl:id>
        <rdfs:label>Lau Island</rdfs:label>
    </owl:NamedIndividual>
    


    <!-- http://purl.obolibrary.org/obo/GAZ_00051691 -->

    <owl:NamedIndividual rdf:about="http://purl.obolibrary.org/obo/GAZ_00051691">
        <obo:RO_0001025 rdf:resource="http://purl.obolibrary.org/obo/GAZ_00051673"/>
        <oboInOwl:hasOBONamespace>GAZ</oboInOwl:hasOBONamespace>
        <oboInOwl:id>GAZ:00051691</oboInOwl:id>
        <rdfs:label>Sawapil Island</rdfs:label>
    </owl:NamedIndividual>
    


    <!-- http://purl.obolibrary.org/obo/GAZ_00051692 -->

    <owl:NamedIndividual rdf:about="http://purl.obolibrary.org/obo/GAZ_00051692">
        <obo:RO_0001025 rdf:resource="http://purl.obolibrary.org/obo/GAZ_00051673"/>
        <oboInOwl:hasOBONamespace>GAZ</oboInOwl:hasOBONamespace>
        <oboInOwl:id>GAZ:00051692</oboInOwl:id>
        <rdfs:label>Menan Island</rdfs:label>
    </owl:NamedIndividual>
    


    <!-- http://purl.obolibrary.org/obo/GAZ_00051693 -->

    <owl:NamedIndividual rdf:about="http://purl.obolibrary.org/obo/GAZ_00051693">
        <obo:RO_0001025 rdf:resource="http://purl.obolibrary.org/obo/GAZ_00051673"/>
        <oboInOwl:hasOBONamespace>GAZ</oboInOwl:hasOBONamespace>
        <oboInOwl:id>GAZ:00051693</oboInOwl:id>
        <rdfs:label>Pelipa Island</rdfs:label>
    </owl:NamedIndividual>
    


    <!-- http://purl.obolibrary.org/obo/GAZ_00051694 -->

    <owl:NamedIndividual rdf:about="http://purl.obolibrary.org/obo/GAZ_00051694">
        <obo:RO_0001025 rdf:resource="http://purl.obolibrary.org/obo/GAZ_00051656"/>
        <oboInOwl:hasOBONamespace>GAZ</oboInOwl:hasOBONamespace>
        <oboInOwl:id>GAZ:00051694</oboInOwl:id>
        <rdfs:label>Somaniat Island</rdfs:label>
    </owl:NamedIndividual>
    


    <!-- http://purl.obolibrary.org/obo/GAZ_00051695 -->

    <owl:NamedIndividual rdf:about="http://purl.obolibrary.org/obo/GAZ_00051695">
        <obo:RO_0001025 rdf:resource="http://purl.obolibrary.org/obo/GAZ_00051654"/>
        <oboInOwl:hasOBONamespace>GAZ</oboInOwl:hasOBONamespace>
        <oboInOwl:id>GAZ:00051695</oboInOwl:id>
        <rdfs:label>Mottum Island</rdfs:label>
    </owl:NamedIndividual>
    


    <!-- http://purl.obolibrary.org/obo/GAZ_00051696 -->

    <owl:NamedIndividual rdf:about="http://purl.obolibrary.org/obo/GAZ_00051696">
        <obo:RO_0001025 rdf:resource="http://purl.obolibrary.org/obo/GAZ_00051656"/>
        <oboInOwl:hasOBONamespace>GAZ</oboInOwl:hasOBONamespace>
        <oboInOwl:id>GAZ:00051696</oboInOwl:id>
        <rdfs:label>Szighwalin Island</rdfs:label>
    </owl:NamedIndividual>
    


    <!-- http://purl.obolibrary.org/obo/GAZ_00051697 -->

    <owl:NamedIndividual rdf:about="http://purl.obolibrary.org/obo/GAZ_00051697">
        <obo:RO_0001025 rdf:resource="http://purl.obolibrary.org/obo/GAZ_00051656"/>
        <oboInOwl:hasOBONamespace>GAZ</oboInOwl:hasOBONamespace>
        <oboInOwl:id>GAZ:00051697</oboInOwl:id>
        <rdfs:label>Pahait Island</rdfs:label>
    </owl:NamedIndividual>
    


    <!-- http://purl.obolibrary.org/obo/GAZ_00051698 -->

    <owl:NamedIndividual rdf:about="http://purl.obolibrary.org/obo/GAZ_00051698">
        <obo:RO_0001025 rdf:resource="http://purl.obolibrary.org/obo/GAZ_00051656"/>
        <oboInOwl:hasOBONamespace>GAZ</oboInOwl:hasOBONamespace>
        <oboInOwl:id>GAZ:00051698</oboInOwl:id>
        <rdfs:label>Hamoha Island</rdfs:label>
    </owl:NamedIndividual>
    


    <!-- http://purl.obolibrary.org/obo/GAZ_00051699 -->

    <owl:NamedIndividual rdf:about="http://purl.obolibrary.org/obo/GAZ_00051699">
        <obo:RO_0001025 rdf:resource="http://purl.obolibrary.org/obo/GAZ_00051656"/>
        <oboInOwl:hasOBONamespace>GAZ</oboInOwl:hasOBONamespace>
        <oboInOwl:id>GAZ:00051699</oboInOwl:id>
        <rdfs:label>Pelleluhu Island</rdfs:label>
    </owl:NamedIndividual>
    


    <!-- http://purl.obolibrary.org/obo/GAZ_00051700 -->

    <owl:NamedIndividual rdf:about="http://purl.obolibrary.org/obo/GAZ_00051700">
        <obo:RO_0001025 rdf:resource="http://purl.obolibrary.org/obo/GAZ_00051656"/>
        <oboInOwl:hasOBONamespace>GAZ</oboInOwl:hasOBONamespace>
        <oboInOwl:id>GAZ:00051700</oboInOwl:id>
        <rdfs:label>Ahaltin Island</rdfs:label>
    </owl:NamedIndividual>
    


    <!-- http://purl.obolibrary.org/obo/GAZ_00051701 -->

    <owl:NamedIndividual rdf:about="http://purl.obolibrary.org/obo/GAZ_00051701">
        <obo:RO_0001025 rdf:resource="http://purl.obolibrary.org/obo/GAZ_00051656"/>
        <oboInOwl:hasOBONamespace>GAZ</oboInOwl:hasOBONamespace>
        <oboInOwl:id>GAZ:00051701</oboInOwl:id>
        <rdfs:label>Pennehan Island</rdfs:label>
    </owl:NamedIndividual>
    


    <!-- http://purl.obolibrary.org/obo/GAZ_00051702 -->

    <owl:NamedIndividual rdf:about="http://purl.obolibrary.org/obo/GAZ_00051702">
        <obo:RO_0001025 rdf:resource="http://purl.obolibrary.org/obo/GAZ_00051656"/>
        <oboInOwl:hasOBONamespace>GAZ</oboInOwl:hasOBONamespace>
        <oboInOwl:id>GAZ:00051702</oboInOwl:id>
        <rdfs:label>Guam Island</rdfs:label>
    </owl:NamedIndividual>
    


    <!-- http://purl.obolibrary.org/obo/GAZ_00051703 -->

    <owl:NamedIndividual rdf:about="http://purl.obolibrary.org/obo/GAZ_00051703">
        <obo:RO_0001025 rdf:resource="http://purl.obolibrary.org/obo/GAZ_00051656"/>
        <oboInOwl:hasOBONamespace>GAZ</oboInOwl:hasOBONamespace>
        <oboInOwl:id>GAZ:00051703</oboInOwl:id>
        <rdfs:label>Moat Island</rdfs:label>
    </owl:NamedIndividual>
    


    <!-- http://purl.obolibrary.org/obo/GAZ_00051704 -->

    <owl:NamedIndividual rdf:about="http://purl.obolibrary.org/obo/GAZ_00051704">
        <obo:RO_0001025 rdf:resource="http://purl.obolibrary.org/obo/GAZ_00051656"/>
        <oboInOwl:hasOBONamespace>GAZ</oboInOwl:hasOBONamespace>
        <oboInOwl:id>GAZ:00051704</oboInOwl:id>
        <rdfs:label>Palitolla Island</rdfs:label>
    </owl:NamedIndividual>
    


    <!-- http://purl.obolibrary.org/obo/GAZ_00051705 -->

    <owl:NamedIndividual rdf:about="http://purl.obolibrary.org/obo/GAZ_00051705">
        <obo:RO_0001025 rdf:resource="http://purl.obolibrary.org/obo/GAZ_00051656"/>
        <oboInOwl:hasOBONamespace>GAZ</oboInOwl:hasOBONamespace>
        <oboInOwl:id>GAZ:00051705</oboInOwl:id>
        <rdfs:label>Bilapalap Island</rdfs:label>
    </owl:NamedIndividual>
    


    <!-- http://purl.obolibrary.org/obo/GAZ_00051706 -->

    <owl:NamedIndividual rdf:about="http://purl.obolibrary.org/obo/GAZ_00051706">
        <obo:RO_0001025 rdf:resource="http://purl.obolibrary.org/obo/GAZ_00051656"/>
        <oboInOwl:hasOBONamespace>GAZ</oboInOwl:hasOBONamespace>
        <oboInOwl:id>GAZ:00051706</oboInOwl:id>
        <rdfs:label>Bircha Island</rdfs:label>
    </owl:NamedIndividual>
    


    <!-- http://purl.obolibrary.org/obo/GAZ_00051707 -->

    <owl:NamedIndividual rdf:about="http://purl.obolibrary.org/obo/GAZ_00051707">
        <obo:RO_0001025 rdf:resource="http://purl.obolibrary.org/obo/GAZ_00051654"/>
        <oboInOwl:hasOBONamespace>GAZ</oboInOwl:hasOBONamespace>
        <oboInOwl:id>GAZ:00051707</oboInOwl:id>
        <rdfs:label>Na Island</rdfs:label>
    </owl:NamedIndividual>
    


    <!-- http://purl.obolibrary.org/obo/GAZ_00051708 -->

    <owl:NamedIndividual rdf:about="http://purl.obolibrary.org/obo/GAZ_00051708">
        <obo:RO_0001025 rdf:resource="http://purl.obolibrary.org/obo/GAZ_00051654"/>
        <oboInOwl:hasOBONamespace>GAZ</oboInOwl:hasOBONamespace>
        <oboInOwl:id>GAZ:00051708</oboInOwl:id>
        <rdfs:label>Laualau island</rdfs:label>
    </owl:NamedIndividual>
    


    <!-- http://purl.obolibrary.org/obo/GAZ_00051709 -->

    <owl:NamedIndividual rdf:about="http://purl.obolibrary.org/obo/GAZ_00051709">
        <obo:RO_0001025 rdf:resource="http://purl.obolibrary.org/obo/GAZ_00051654"/>
        <oboInOwl:hasOBONamespace>GAZ</oboInOwl:hasOBONamespace>
        <oboInOwl:id>GAZ:00051709</oboInOwl:id>
        <rdfs:label>Tall Island</rdfs:label>
    </owl:NamedIndividual>
    


    <!-- http://purl.obolibrary.org/obo/GAZ_00051710 -->

    <owl:NamedIndividual rdf:about="http://purl.obolibrary.org/obo/GAZ_00051710">
        <obo:RO_0001025 rdf:resource="http://purl.obolibrary.org/obo/GAZ_00051654"/>
        <oboInOwl:hasOBONamespace>GAZ</oboInOwl:hasOBONamespace>
        <oboInOwl:id>GAZ:00051710</oboInOwl:id>
        <rdfs:label>Sa Island</rdfs:label>
    </owl:NamedIndividual>
    


    <!-- http://purl.obolibrary.org/obo/GAZ_00051711 -->

    <owl:NamedIndividual rdf:about="http://purl.obolibrary.org/obo/GAZ_00051711">
        <obo:RO_0001025 rdf:resource="http://purl.obolibrary.org/obo/GAZ_00051654"/>
        <oboInOwl:hasOBONamespace>GAZ</oboInOwl:hasOBONamespace>
        <oboInOwl:id>GAZ:00051711</oboInOwl:id>
        <rdfs:label>Kat Island</rdfs:label>
    </owl:NamedIndividual>
    


    <!-- http://purl.obolibrary.org/obo/GAZ_00051712 -->

    <owl:NamedIndividual rdf:about="http://purl.obolibrary.org/obo/GAZ_00051712">
        <rdf:type rdf:resource="http://purl.obolibrary.org/obo/ENVO_00000220"/>
        <obo:RO_0001025 rdf:resource="http://purl.obolibrary.org/obo/GAZ_00016822"/>
        <obo:IAO_0000115>An island group that lies 162 km west of the island of Manus (in the Admiralty Islands) and 73 km southeast of the Ninigo Islands; the mouth of the Sepik River on the PNG mainland is situated 250 km to the southwest.</obo:IAO_0000115>
        <oboInOwl:hasOBONamespace>GAZ</oboInOwl:hasOBONamespace>
        <oboInOwl:id>GAZ:00051712</oboInOwl:id>
        <rdfs:label>Hermit Islands</rdfs:label>
    </owl:NamedIndividual>
    


    <!-- http://purl.obolibrary.org/obo/GAZ_00051713 -->

    <owl:NamedIndividual rdf:about="http://purl.obolibrary.org/obo/GAZ_00051713">
        <obo:RO_0001025 rdf:resource="http://purl.obolibrary.org/obo/GAZ_00051712"/>
        <obo:IAO_0000115>The lagoon of the Hermit reef complex.</obo:IAO_0000115>
        <oboInOwl:hasOBONamespace>GAZ</oboInOwl:hasOBONamespace>
        <oboInOwl:id>GAZ:00051713</oboInOwl:id>
        <rdfs:label>Hermit Lagoon</rdfs:label>
    </owl:NamedIndividual>
    


    <!-- http://purl.obolibrary.org/obo/GAZ_00051714 -->

    <owl:NamedIndividual rdf:about="http://purl.obolibrary.org/obo/GAZ_00051714">
        <obo:RO_0001025 rdf:resource="http://purl.obolibrary.org/obo/GAZ_00051712"/>
        <obo:IAO_0000115>An island-barrier reef complex.</obo:IAO_0000115>
        <oboInOwl:hasOBONamespace>GAZ</oboInOwl:hasOBONamespace>
        <oboInOwl:id>GAZ:00051714</oboInOwl:id>
        <rdfs:label>Hermit Reef</rdfs:label>
    </owl:NamedIndividual>
    


    <!-- http://purl.obolibrary.org/obo/GAZ_00051715 -->

    <owl:NamedIndividual rdf:about="http://purl.obolibrary.org/obo/GAZ_00051715">
        <obo:RO_0001025 rdf:resource="http://purl.obolibrary.org/obo/GAZ_00051713"/>
        <oboInOwl:hasOBONamespace>GAZ</oboInOwl:hasOBONamespace>
        <oboInOwl:id>GAZ:00051715</oboInOwl:id>
        <rdfs:label>Jalun Island</rdfs:label>
    </owl:NamedIndividual>
    


    <!-- http://purl.obolibrary.org/obo/GAZ_00051716 -->

    <owl:NamedIndividual rdf:about="http://purl.obolibrary.org/obo/GAZ_00051716">
        <obo:RO_0001025 rdf:resource="http://purl.obolibrary.org/obo/GAZ_00051713"/>
        <oboInOwl:hasOBONamespace>GAZ</oboInOwl:hasOBONamespace>
        <oboInOwl:id>GAZ:00051716</oboInOwl:id>
        <rdfs:label>Maron Island</rdfs:label>
    </owl:NamedIndividual>
    


    <!-- http://purl.obolibrary.org/obo/GAZ_00051717 -->

    <owl:NamedIndividual rdf:about="http://purl.obolibrary.org/obo/GAZ_00051717">
        <obo:RO_0001025 rdf:resource="http://purl.obolibrary.org/obo/GAZ_00051713"/>
        <oboInOwl:hasOBONamespace>GAZ</oboInOwl:hasOBONamespace>
        <oboInOwl:id>GAZ:00051717</oboInOwl:id>
        <rdfs:label>South Gochonsipi Island</rdfs:label>
    </owl:NamedIndividual>
    


    <!-- http://purl.obolibrary.org/obo/GAZ_00051718 -->

    <owl:NamedIndividual rdf:about="http://purl.obolibrary.org/obo/GAZ_00051718">
        <obo:RO_0001025 rdf:resource="http://purl.obolibrary.org/obo/GAZ_00051713"/>
        <oboInOwl:hasOBONamespace>GAZ</oboInOwl:hasOBONamespace>
        <oboInOwl:id>GAZ:00051718</oboInOwl:id>
        <rdfs:label>Tset Island</rdfs:label>
    </owl:NamedIndividual>
    


    <!-- http://purl.obolibrary.org/obo/GAZ_00051719 -->

    <owl:NamedIndividual rdf:about="http://purl.obolibrary.org/obo/GAZ_00051719">
        <obo:RO_0001025 rdf:resource="http://purl.obolibrary.org/obo/GAZ_00051713"/>
        <oboInOwl:hasOBONamespace>GAZ</oboInOwl:hasOBONamespace>
        <oboInOwl:id>GAZ:00051719</oboInOwl:id>
        <rdfs:label>Luf Island</rdfs:label>
    </owl:NamedIndividual>
    


    <!-- http://purl.obolibrary.org/obo/GAZ_00051720 -->

    <owl:NamedIndividual rdf:about="http://purl.obolibrary.org/obo/GAZ_00051720">
        <obo:RO_0001025 rdf:resource="http://purl.obolibrary.org/obo/GAZ_00051713"/>
        <oboInOwl:hasOBONamespace>GAZ</oboInOwl:hasOBONamespace>
        <oboInOwl:id>GAZ:00051720</oboInOwl:id>
        <rdfs:label>North Gochonsipi Island</rdfs:label>
    </owl:NamedIndividual>
    


    <!-- http://purl.obolibrary.org/obo/GAZ_00051721 -->

    <owl:NamedIndividual rdf:about="http://purl.obolibrary.org/obo/GAZ_00051721">
        <obo:RO_0001025 rdf:resource="http://purl.obolibrary.org/obo/GAZ_00051713"/>
        <oboInOwl:hasOBONamespace>GAZ</oboInOwl:hasOBONamespace>
        <oboInOwl:id>GAZ:00051721</oboInOwl:id>
        <rdfs:label>Akib Island</rdfs:label>
    </owl:NamedIndividual>
    


    <!-- http://purl.obolibrary.org/obo/GAZ_00051722 -->

    <owl:NamedIndividual rdf:about="http://purl.obolibrary.org/obo/GAZ_00051722">
        <obo:RO_0001025 rdf:resource="http://purl.obolibrary.org/obo/GAZ_00051714"/>
        <oboInOwl:hasOBONamespace>GAZ</oboInOwl:hasOBONamespace>
        <oboInOwl:id>GAZ:00051722</oboInOwl:id>
        <rdfs:label>Pianau Island</rdfs:label>
    </owl:NamedIndividual>
    


    <!-- http://purl.obolibrary.org/obo/GAZ_00051723 -->

    <owl:NamedIndividual rdf:about="http://purl.obolibrary.org/obo/GAZ_00051723">
        <obo:RO_0001025 rdf:resource="http://purl.obolibrary.org/obo/GAZ_00051714"/>
        <oboInOwl:hasOBONamespace>GAZ</oboInOwl:hasOBONamespace>
        <oboInOwl:id>GAZ:00051723</oboInOwl:id>
        <rdfs:label>Pemei Island</rdfs:label>
    </owl:NamedIndividual>
    


    <!-- http://purl.obolibrary.org/obo/GAZ_00051724 -->

    <owl:NamedIndividual rdf:about="http://purl.obolibrary.org/obo/GAZ_00051724">
        <obo:RO_0001025 rdf:resource="http://purl.obolibrary.org/obo/GAZ_00051714"/>
        <oboInOwl:hasOBONamespace>GAZ</oboInOwl:hasOBONamespace>
        <oboInOwl:id>GAZ:00051724</oboInOwl:id>
        <rdfs:label>Leabon Island</rdfs:label>
    </owl:NamedIndividual>
    


    <!-- http://purl.obolibrary.org/obo/GAZ_00051725 -->

    <owl:NamedIndividual rdf:about="http://purl.obolibrary.org/obo/GAZ_00051725">
        <obo:RO_0001025 rdf:resource="http://purl.obolibrary.org/obo/GAZ_00051714"/>
        <oboInOwl:hasOBONamespace>GAZ</oboInOwl:hasOBONamespace>
        <oboInOwl:id>GAZ:00051725</oboInOwl:id>
        <rdfs:label>Makan Island</rdfs:label>
    </owl:NamedIndividual>
    


    <!-- http://purl.obolibrary.org/obo/GAZ_00051726 -->

    <owl:NamedIndividual rdf:about="http://purl.obolibrary.org/obo/GAZ_00051726">
        <obo:RO_0001025 rdf:resource="http://purl.obolibrary.org/obo/GAZ_00051714"/>
        <oboInOwl:hasOBONamespace>GAZ</oboInOwl:hasOBONamespace>
        <oboInOwl:id>GAZ:00051726</oboInOwl:id>
        <rdfs:label>Tatahau Island</rdfs:label>
    </owl:NamedIndividual>
    


    <!-- http://purl.obolibrary.org/obo/GAZ_00051727 -->

    <owl:NamedIndividual rdf:about="http://purl.obolibrary.org/obo/GAZ_00051727">
        <obo:RO_0001025 rdf:resource="http://purl.obolibrary.org/obo/GAZ_00051714"/>
        <oboInOwl:hasOBONamespace>GAZ</oboInOwl:hasOBONamespace>
        <oboInOwl:id>GAZ:00051727</oboInOwl:id>
        <rdfs:label>Kenai Island</rdfs:label>
    </owl:NamedIndividual>
    


    <!-- http://purl.obolibrary.org/obo/GAZ_00051728 -->

    <owl:NamedIndividual rdf:about="http://purl.obolibrary.org/obo/GAZ_00051728">
        <obo:RO_0001025 rdf:resource="http://purl.obolibrary.org/obo/GAZ_00051714"/>
        <oboInOwl:hasOBONamespace>GAZ</oboInOwl:hasOBONamespace>
        <oboInOwl:id>GAZ:00051728</oboInOwl:id>
        <rdfs:label>Mono Island</rdfs:label>
    </owl:NamedIndividual>
    


    <!-- http://purl.obolibrary.org/obo/GAZ_00051729 -->

    <owl:NamedIndividual rdf:about="http://purl.obolibrary.org/obo/GAZ_00051729">
        <obo:RO_0001025 rdf:resource="http://purl.obolibrary.org/obo/GAZ_00051714"/>
        <oboInOwl:hasOBONamespace>GAZ</oboInOwl:hasOBONamespace>
        <oboInOwl:id>GAZ:00051729</oboInOwl:id>
        <rdfs:label>Amot Island</rdfs:label>
    </owl:NamedIndividual>
    


    <!-- http://purl.obolibrary.org/obo/GAZ_00051730 -->

    <owl:NamedIndividual rdf:about="http://purl.obolibrary.org/obo/GAZ_00051730">
        <obo:RO_0001025 rdf:resource="http://purl.obolibrary.org/obo/GAZ_00051714"/>
        <oboInOwl:hasOBONamespace>GAZ</oboInOwl:hasOBONamespace>
        <oboInOwl:id>GAZ:00051730</oboInOwl:id>
        <rdfs:label>Kocheran Island</rdfs:label>
    </owl:NamedIndividual>
    


    <!-- http://purl.obolibrary.org/obo/GAZ_00051731 -->

    <owl:NamedIndividual rdf:about="http://purl.obolibrary.org/obo/GAZ_00051731">
        <obo:RO_0001025 rdf:resource="http://purl.obolibrary.org/obo/GAZ_00051714"/>
        <oboInOwl:hasOBONamespace>GAZ</oboInOwl:hasOBONamespace>
        <oboInOwl:id>GAZ:00051731</oboInOwl:id>
        <rdfs:label>Pechu Island</rdfs:label>
    </owl:NamedIndividual>
    


    <!-- http://purl.obolibrary.org/obo/GAZ_00051732 -->

    <owl:NamedIndividual rdf:about="http://purl.obolibrary.org/obo/GAZ_00051732">
        <obo:RO_0001025 rdf:resource="http://purl.obolibrary.org/obo/GAZ_00016822"/>
        <oboInOwl:hasOBONamespace>GAZ</oboInOwl:hasOBONamespace>
        <oboInOwl:id>GAZ:00051732</oboInOwl:id>
        <rdfs:label>Sae Islands</rdfs:label>
    </owl:NamedIndividual>
    


    <!-- http://purl.obolibrary.org/obo/GAZ_00051733 -->

    <owl:NamedIndividual rdf:about="http://purl.obolibrary.org/obo/GAZ_00051733">
        <obo:RO_0001025 rdf:resource="http://purl.obolibrary.org/obo/GAZ_00051732"/>
        <oboInOwl:hasOBONamespace>GAZ</oboInOwl:hasOBONamespace>
        <oboInOwl:id>GAZ:00051733</oboInOwl:id>
        <rdfs:label>Sae Island</rdfs:label>
    </owl:NamedIndividual>
    


    <!-- http://purl.obolibrary.org/obo/GAZ_00051734 -->

    <owl:NamedIndividual rdf:about="http://purl.obolibrary.org/obo/GAZ_00051734">
        <rdf:type rdf:resource="http://purl.obolibrary.org/obo/ENVO_00000220"/>
        <obo:RO_0001025 rdf:resource="http://purl.obolibrary.org/obo/GAZ_00016822"/>
        <obo:IAO_0000115>An island group.</obo:IAO_0000115>
        <oboInOwl:hasOBONamespace>GAZ</oboInOwl:hasOBONamespace>
        <oboInOwl:id>GAZ:00051734</oboInOwl:id>
        <rdfs:label>Kaniet Islands</rdfs:label>
    </owl:NamedIndividual>
    


    <!-- http://purl.obolibrary.org/obo/GAZ_00051735 -->

    <owl:NamedIndividual rdf:about="http://purl.obolibrary.org/obo/GAZ_00051735">
        <obo:RO_0001025 rdf:resource="http://purl.obolibrary.org/obo/GAZ_00051734"/>
        <oboInOwl:hasOBONamespace>GAZ</oboInOwl:hasOBONamespace>
        <oboInOwl:id>GAZ:00051735</oboInOwl:id>
        <rdfs:label>Tatak Island</rdfs:label>
    </owl:NamedIndividual>
    


    <!-- http://purl.obolibrary.org/obo/GAZ_00051736 -->

    <owl:NamedIndividual rdf:about="http://purl.obolibrary.org/obo/GAZ_00051736">
        <obo:RO_0001025 rdf:resource="http://purl.obolibrary.org/obo/GAZ_00051734"/>
        <oboInOwl:hasOBONamespace>GAZ</oboInOwl:hasOBONamespace>
        <oboInOwl:id>GAZ:00051736</oboInOwl:id>
        <rdfs:label>Vasan Island</rdfs:label>
    </owl:NamedIndividual>
    


    <!-- http://purl.obolibrary.org/obo/GAZ_00051737 -->

    <owl:NamedIndividual rdf:about="http://purl.obolibrary.org/obo/GAZ_00051737">
        <obo:RO_0001025 rdf:resource="http://purl.obolibrary.org/obo/GAZ_00051734"/>
        <oboInOwl:hasOBONamespace>GAZ</oboInOwl:hasOBONamespace>
        <oboInOwl:id>GAZ:00051737</oboInOwl:id>
        <rdfs:label>Taling Island</rdfs:label>
    </owl:NamedIndividual>
    


    <!-- http://purl.obolibrary.org/obo/GAZ_00051738 -->

    <owl:NamedIndividual rdf:about="http://purl.obolibrary.org/obo/GAZ_00051738">
        <obo:RO_0001025 rdf:resource="http://purl.obolibrary.org/obo/GAZ_00051734"/>
        <oboInOwl:hasOBONamespace>GAZ</oboInOwl:hasOBONamespace>
        <oboInOwl:id>GAZ:00051738</oboInOwl:id>
        <rdfs:label>Suf Island</rdfs:label>
    </owl:NamedIndividual>
    


    <!-- http://purl.obolibrary.org/obo/GAZ_00051740 -->

    <owl:NamedIndividual rdf:about="http://purl.obolibrary.org/obo/GAZ_00051740">
        <obo:RO_0001025 rdf:resource="http://purl.obolibrary.org/obo/GAZ_00118096"/>
        <obo:IAO_0000115>A small group of islands in Papua New Guinea.</obo:IAO_0000115>
        <oboInOwl:hasOBONamespace>GAZ</oboInOwl:hasOBONamespace>
        <oboInOwl:id>GAZ:00051740</oboInOwl:id>
        <rdfs:label>Green Islands</rdfs:label>
    </owl:NamedIndividual>
    


    <!-- http://purl.obolibrary.org/obo/GAZ_00051777 -->

    <owl:NamedIndividual rdf:about="http://purl.obolibrary.org/obo/GAZ_00051777">
        <obo:RO_0001025 rdf:resource="http://purl.obolibrary.org/obo/GAZ_00005266"/>
        <obo:IAO_0000115>A group of six small volcanic islands in the province of East Sepik in Papua New Guinea, north of the island of New Guinea. The group is also called Eastern Schouten Islands or Le Maire Islands to separate it from unrelated Schouten Islands in Indonesia.</obo:IAO_0000115>
        <oboInOwl:hasOBONamespace>GAZ</oboInOwl:hasOBONamespace>
        <oboInOwl:id>GAZ:00051777</oboInOwl:id>
        <rdfs:label>Schouten Islands</rdfs:label>
    </owl:NamedIndividual>
    


    <!-- http://purl.obolibrary.org/obo/GAZ_00051778 -->

    <owl:NamedIndividual rdf:about="http://purl.obolibrary.org/obo/GAZ_00051778">
        <obo:RO_0001025 rdf:resource="http://purl.obolibrary.org/obo/GAZ_00051777"/>
        <obo:IAO_0000115>An island that is the summit of a mostly submerged volcano that is one of the more active in Papua New Guinea. Bam is the SE-most of the Schouten Islands, and lies off the coast of New Guinea, about 40 km NNE of the mouth of the Sepik River. A steep-walled summit crater that is 300 m wide and 180 m deep is the source of Bam&apos;s recent eruptions, which have kept the upper half of the cone sparsely vegetated. A NE-trending landslide scarp extends across the upper part of the andesitic volcano from the SW coast; the younger cone has formed inside this scarp on the east side of the island. A lava platform on the north flank supports the small island&apos;s only villages.</obo:IAO_0000115>
        <oboInOwl:hasOBONamespace>GAZ</oboInOwl:hasOBONamespace>
        <oboInOwl:id>GAZ:00051778</oboInOwl:id>
        <rdfs:label>Bam Island</rdfs:label>
    </owl:NamedIndividual>
    


    <!-- http://purl.obolibrary.org/obo/GAZ_00051779 -->

    <owl:NamedIndividual rdf:about="http://purl.obolibrary.org/obo/GAZ_00051779">
        <obo:RO_0001025 rdf:resource="http://purl.obolibrary.org/obo/GAZ_00051777"/>
        <obo:IAO_0000115>One of the Schouten Islands.</obo:IAO_0000115>
        <oboInOwl:hasOBONamespace>GAZ</oboInOwl:hasOBONamespace>
        <oboInOwl:id>GAZ:00051779</oboInOwl:id>
        <rdfs:label>Koil Island</rdfs:label>
    </owl:NamedIndividual>
    


    <!-- http://purl.obolibrary.org/obo/GAZ_00051780 -->

    <owl:NamedIndividual rdf:about="http://purl.obolibrary.org/obo/GAZ_00051780">
        <obo:RO_0001025 rdf:resource="http://purl.obolibrary.org/obo/GAZ_00051777"/>
        <obo:IAO_0000115>One of the Schouten Islands.</obo:IAO_0000115>
        <oboInOwl:hasOBONamespace>GAZ</oboInOwl:hasOBONamespace>
        <oboInOwl:id>GAZ:00051780</oboInOwl:id>
        <rdfs:label>Wei Island</rdfs:label>
    </owl:NamedIndividual>
    


    <!-- http://purl.obolibrary.org/obo/GAZ_00051781 -->

    <owl:NamedIndividual rdf:about="http://purl.obolibrary.org/obo/GAZ_00051781">
        <obo:RO_0001025 rdf:resource="http://purl.obolibrary.org/obo/GAZ_00051777"/>
        <obo:IAO_0000115>An island that is the emergent summit of a Bismarck Sea stratovolcano of Holocene age. Kadovar is part of the Schouten Islands, and lies off the coast of New Guinea, about 25 km north of the mouth of the Sepik River. The village of Gewai is perched on the crater rim. A 365 m high lava dome forming the high point of the andesitic volcano fills an arcuate landslide scarp that is open to the south. Thick lava flows with columnar jointing forms low cliffs along the coast. The youthful island lacks fringing or offshore reefs.</obo:IAO_0000115>
        <oboInOwl:hasOBONamespace>GAZ</oboInOwl:hasOBONamespace>
        <oboInOwl:id>GAZ:00051781</oboInOwl:id>
        <rdfs:label>Kadovar Island</rdfs:label>
    </owl:NamedIndividual>
    


    <!-- http://purl.obolibrary.org/obo/GAZ_00051782 -->

    <owl:NamedIndividual rdf:about="http://purl.obolibrary.org/obo/GAZ_00051782">
        <obo:RO_0001025 rdf:resource="http://purl.obolibrary.org/obo/GAZ_00051777"/>
        <obo:IAO_0000115>A small forested island of the northern coast of Papua New Guinea about 30 km offshore from Cape Girgir and is considered part of the Schouten Islands. It contains lava flows with well-defined flow fronts. A weak thermal area is located on the west coast. Most eruptive activity at the andesitic-dacitic volcano originated from a thickly wooded summit crater about 800 m in diameter, although a lava dome may be present on a ridge to the west, and a small satellite cone occurs along the SW coast.</obo:IAO_0000115>
        <oboInOwl:hasOBONamespace>GAZ</oboInOwl:hasOBONamespace>
        <oboInOwl:id>GAZ:00051782</oboInOwl:id>
        <rdfs:label>Blup Blup Island</rdfs:label>
    </owl:NamedIndividual>
    


    <!-- http://purl.obolibrary.org/obo/GAZ_00051783 -->

    <owl:NamedIndividual rdf:about="http://purl.obolibrary.org/obo/GAZ_00051783">
        <obo:RO_0001025 rdf:resource="http://purl.obolibrary.org/obo/GAZ_00051777"/>
        <obo:IAO_0000115>One of the Schouten Islands.</obo:IAO_0000115>
        <oboInOwl:hasOBONamespace>GAZ</oboInOwl:hasOBONamespace>
        <oboInOwl:id>GAZ:00051783</oboInOwl:id>
        <rdfs:label>Vokeo Island</rdfs:label>
    </owl:NamedIndividual>
    


    <!-- http://purl.obolibrary.org/obo/GAZ_00053876 -->

    <owl:NamedIndividual rdf:about="http://purl.obolibrary.org/obo/GAZ_00053876">
        <rdf:type rdf:resource="http://purl.obolibrary.org/obo/ENVO_00000354"/>
        <obo:RO_0001025 rdf:resource="http://purl.obolibrary.org/obo/GAZ_00007179"/>
        <obo:IAO_0000115>A volcanic complex located in the Admiralty Islands north of Papua New Guinea, consists of a series of overlapping Quaternary cones formed by rhyolitic lava flows and pyroclastic materials on Lou and Tuluman Islands. Volcanism is aligned on a curved arc extending through the 12 km-long Lou Island, which may represent an incipient caldera ring fracture. The historically active Tuluman Islands, 1.5 km south of Lou Island, were formed during a 1953-1957 eruption. Pam Lin and Pam Mandian Islands farther to the SE along the same arc contain fresh rhyolitic obsidian similar to that found on Tuluman.</obo:IAO_0000115>
        <oboInOwl:hasOBONamespace>GAZ</oboInOwl:hasOBONamespace>
        <oboInOwl:id>GAZ:00053876</oboInOwl:id>
        <rdfs:label>Saint Andrew Strait Volcanic Complex</rdfs:label>
    </owl:NamedIndividual>
    


    <!-- http://purl.obolibrary.org/obo/GAZ_00053877 -->

    <owl:NamedIndividual rdf:about="http://purl.obolibrary.org/obo/GAZ_00053877">
        <obo:RO_0001025 rdf:resource="http://purl.obolibrary.org/obo/GAZ_00005193"/>
        <obo:IAO_0000115>An island in the Bismark Sea. It consists of a large basaltic-andesitic cone with a summit crater open to the north whose rim extends to the island&apos;s east coast. The crater of the basaltic older cone is filled by two steep-sided andesitic lava domes, the highest of which forms the 240-m high point of the island. A third lava dome, separated from the eastern cone by a low saddle, forms a peninsula on the western side of the island.</obo:IAO_0000115>
        <oboInOwl:hasOBONamespace>GAZ</oboInOwl:hasOBONamespace>
        <oboInOwl:id>GAZ:00053877</oboInOwl:id>
        <rdfs:label>Boisa Island</rdfs:label>
    </owl:NamedIndividual>
    


    <!-- http://purl.obolibrary.org/obo/GAZ_00053878 -->

    <owl:NamedIndividual rdf:about="http://purl.obolibrary.org/obo/GAZ_00053878">
        <obo:RO_0001025 rdf:resource="http://purl.obolibrary.org/obo/GAZ_00005193"/>
        <obo:RO_0001025 rdf:resource="http://purl.obolibrary.org/obo/GAZ_00005198"/>
        <obo:IAO_0000115>An island located in the Bismarck Sea across the Stephan Strait from the northeast coast of mainland Papua New Guinea. Four large radial valleys extend from the unvegetated summit of the conical 1807 m high basaltic-andesitic stratovolcano to its lower flanks. These &quot;avalanche valleys,&quot; regularly spaced 90 degrees apart, channel lava flows and pyroclastic avalanches that have sometimes reached the coast. Five small satellitic centers are located near the island&apos;s shoreline on the northern, southern and western sides. Two summit craters are present; both are active, although most historical eruptions have originated from the southern crater, concentrating eruptive products during much of the past century into the SE avalanche valley.</obo:IAO_0000115>
        <oboInOwl:hasOBONamespace>GAZ</oboInOwl:hasOBONamespace>
        <oboInOwl:id>GAZ:00053878</oboInOwl:id>
        <rdfs:label>Manam Island</rdfs:label>
    </owl:NamedIndividual>
    


    <!-- http://purl.obolibrary.org/obo/GAZ_00053879 -->

    <owl:NamedIndividual rdf:about="http://purl.obolibrary.org/obo/GAZ_00053879">
        <obo:RO_0001025 rdf:resource="http://purl.obolibrary.org/obo/GAZ_00005193"/>
        <obo:RO_0001025 rdf:resource="http://purl.obolibrary.org/obo/GAZ_00005198"/>
        <obo:IAO_0000115>An island in the Bismark Sea. An island that is truncated by two nested summit calderas. The 5.5 km wide outer caldera was formed during one or more eruptions, the last of which occurred 9000 years ago. The eccentric 3.2 km wide inner caldera was formed sometime between 1500 and 800 years ago. Parasitic cones are present on the northern and southern flanks of basaltic-to-andesitic Karkar volcano; a linear array of small cones extends from the northern rim of the outer caldera nearly to the coast.</obo:IAO_0000115>
        <oboInOwl:hasOBONamespace>GAZ</oboInOwl:hasOBONamespace>
        <oboInOwl:id>GAZ:00053879</oboInOwl:id>
        <rdfs:label>Karkar Island</rdfs:label>
    </owl:NamedIndividual>
    


    <!-- http://purl.obolibrary.org/obo/GAZ_00053880 -->

    <owl:NamedIndividual rdf:about="http://purl.obolibrary.org/obo/GAZ_00053880">
        <obo:RO_0001025 rdf:resource="http://purl.obolibrary.org/obo/GAZ_00005193"/>
        <obo:IAO_0000115>An island in the Bismark Sea.</obo:IAO_0000115>
        <oboInOwl:hasOBONamespace>GAZ</oboInOwl:hasOBONamespace>
        <oboInOwl:id>GAZ:00053880</oboInOwl:id>
        <rdfs:label>Yomba Island</rdfs:label>
    </owl:NamedIndividual>
    


    <!-- http://purl.obolibrary.org/obo/GAZ_00053881 -->

    <owl:NamedIndividual rdf:about="http://purl.obolibrary.org/obo/GAZ_00053881">
        <obo:RO_0001025 rdf:resource="http://purl.obolibrary.org/obo/GAZ_00005193"/>
        <obo:IAO_0000115>A small crescent-shaped volcanic island 100 km northeast of New Guinea, situated between Umboi Island and Sakar Island. Prior to 1888, Ritter Island was a steep-sided, nearly circular island about 780 m high. The current small, 140 m high island is a topographically insignificant, 1900-m-long arcuate feature between Umboi and Sakar Islands. Several historical explosive eruptions had been recorded prior to 1888, when large-scale slope failure destroyed the summit of the conical basaltic-andesitic volcano, leaving the arcuate 140 m high island remnant with a steep west-facing scarp that descends below sea level. Devastating tsunamis were produced by the collapse and swept the coast of Papua New Guinea and offshore islands. Two minor post-collapse explosive eruptions, during 1972 and 1974, occurred offshore within the largely submarine 3.5 x 4.5 km breached depression formed by the collapse.</obo:IAO_0000115>
        <oboInOwl:hasOBONamespace>GAZ</oboInOwl:hasOBONamespace>
        <oboInOwl:id>GAZ:00053881</oboInOwl:id>
        <rdfs:label>Ritter Island</rdfs:label>
    </owl:NamedIndividual>
    


    <!-- http://purl.obolibrary.org/obo/GAZ_00053882 -->

    <owl:NamedIndividual rdf:about="http://purl.obolibrary.org/obo/GAZ_00053882">
        <obo:RO_0001025 rdf:resource="http://purl.obolibrary.org/obo/GAZ_00005193"/>
        <obo:RO_0001025 rdf:resource="http://purl.obolibrary.org/obo/GAZ_00005198"/>
        <obo:IAO_0000115>A volcanic island north of Papua New Guinea. It is separated from the island of New Guinea by Vitiaz Strait. An island dominated by two steep-sided stratovolcanoes, Mount Reaumur in the north and Cerisy Peak in the south. Collapse of the basaltic-andesitic volcanic complex produced a large 10 x 12.5 km caldera, now filled by Lake Wisdom. Caldera formation occurred during at least three major explosive eruptions, about 16,000, 4000, and 300 years ago.</obo:IAO_0000115>
        <oboInOwl:hasOBONamespace>GAZ</oboInOwl:hasOBONamespace>
        <oboInOwl:id>GAZ:00053882</oboInOwl:id>
        <rdfs:label>Long Island</rdfs:label>
    </owl:NamedIndividual>
    


    <!-- http://purl.obolibrary.org/obo/GAZ_00053883 -->

    <owl:NamedIndividual rdf:about="http://purl.obolibrary.org/obo/GAZ_00053883">
        <obo:RO_0001025 rdf:resource="http://purl.obolibrary.org/obo/GAZ_00053882"/>
        <obo:IAO_0000115>A stratovolcano.</obo:IAO_0000115>
        <oboInOwl:hasOBONamespace>GAZ</oboInOwl:hasOBONamespace>
        <oboInOwl:id>GAZ:00053883</oboInOwl:id>
        <rdfs:label>Cerisy Peak</rdfs:label>
    </owl:NamedIndividual>
    


    <!-- http://purl.obolibrary.org/obo/GAZ_00053884 -->

    <owl:NamedIndividual rdf:about="http://purl.obolibrary.org/obo/GAZ_00053884">
        <obo:RO_0001025 rdf:resource="http://purl.obolibrary.org/obo/GAZ_00053882"/>
        <obo:IAO_0000115>A stratovolcano.</obo:IAO_0000115>
        <oboInOwl:hasOBONamespace>GAZ</oboInOwl:hasOBONamespace>
        <oboInOwl:id>GAZ:00053884</oboInOwl:id>
        <rdfs:label>Mount Reaumur</rdfs:label>
    </owl:NamedIndividual>
    


    <!-- http://purl.obolibrary.org/obo/GAZ_00053885 -->

    <owl:NamedIndividual rdf:about="http://purl.obolibrary.org/obo/GAZ_00053885">
        <obo:RO_0001025 rdf:resource="http://purl.obolibrary.org/obo/GAZ_00005193"/>
        <obo:IAO_0000115>A submerged reef formation of the southwestern Bismarck Sea located 50 km northwest from Long Island and 77 km southeast from karkar; its closest neighbour is the small Crown Island, 30 km to the southwest. Perhaps the site of a former island, that resulted from a submarine volcano.</obo:IAO_0000115>
        <oboInOwl:hasOBONamespace>GAZ</oboInOwl:hasOBONamespace>
        <oboInOwl:id>GAZ:00053885</oboInOwl:id>
        <rdfs:label>Hankow Reef</rdfs:label>
    </owl:NamedIndividual>
    


    <!-- http://purl.obolibrary.org/obo/GAZ_00053886 -->

    <owl:NamedIndividual rdf:about="http://purl.obolibrary.org/obo/GAZ_00053886">
        <obo:RO_0001025 rdf:resource="http://purl.obolibrary.org/obo/GAZ_00051283"/>
        <oboInOwl:hasOBONamespace>GAZ</oboInOwl:hasOBONamespace>
        <oboInOwl:id>GAZ:00053886</oboInOwl:id>
        <rdfs:label>Soal Cone</rdfs:label>
    </owl:NamedIndividual>
    


    <!-- http://purl.obolibrary.org/obo/GAZ_00053887 -->

    <owl:NamedIndividual rdf:about="http://purl.obolibrary.org/obo/GAZ_00053887">
        <obo:RO_0001025 rdf:resource="http://purl.obolibrary.org/obo/GAZ_00051283"/>
        <oboInOwl:hasOBONamespace>GAZ</oboInOwl:hasOBONamespace>
        <oboInOwl:id>GAZ:00053887</oboInOwl:id>
        <rdfs:label>Talo Cone</rdfs:label>
    </owl:NamedIndividual>
    


    <!-- http://purl.obolibrary.org/obo/GAZ_00053888 -->

    <owl:NamedIndividual rdf:about="http://purl.obolibrary.org/obo/GAZ_00053888">
        <obo:RO_0001025 rdf:resource="http://purl.obolibrary.org/obo/GAZ_00051283"/>
        <oboInOwl:hasOBONamespace>GAZ</oboInOwl:hasOBONamespace>
        <oboInOwl:id>GAZ:00053888</oboInOwl:id>
        <rdfs:label>Barik Cone</rdfs:label>
    </owl:NamedIndividual>
    


    <!-- http://purl.obolibrary.org/obo/GAZ_00053889 -->

    <owl:NamedIndividual rdf:about="http://purl.obolibrary.org/obo/GAZ_00053889">
        <obo:RO_0001025 rdf:resource="http://purl.obolibrary.org/obo/GAZ_00053891"/>
        <obo:IAO_0000115>A mountain range on Gazelle Peninsula, New Britain, Papua New Guinea.</obo:IAO_0000115>
        <oboInOwl:hasOBONamespace>GAZ</oboInOwl:hasOBONamespace>
        <oboInOwl:id>GAZ:00053889</oboInOwl:id>
        <rdfs:label>Baining Mountains</rdfs:label>
    </owl:NamedIndividual>
    


    <!-- http://purl.obolibrary.org/obo/GAZ_00053890 -->

    <owl:NamedIndividual rdf:about="http://purl.obolibrary.org/obo/GAZ_00053890">
        <obo:RO_0001025 rdf:resource="http://purl.obolibrary.org/obo/GAZ_00053889"/>
        <obo:IAO_0000115>The highest peak of the Baining Mountains.</obo:IAO_0000115>
        <oboInOwl:hasOBONamespace>GAZ</oboInOwl:hasOBONamespace>
        <oboInOwl:id>GAZ:00053890</oboInOwl:id>
        <rdfs:label>Mount Sinewit</rdfs:label>
    </owl:NamedIndividual>
    


    <!-- http://purl.obolibrary.org/obo/GAZ_00053891 -->

    <owl:NamedIndividual rdf:about="http://purl.obolibrary.org/obo/GAZ_00053891">
        <obo:RO_0001025 rdf:resource="http://purl.obolibrary.org/obo/GAZ_00005189"/>
        <obo:RO_0001025 rdf:resource="http://purl.obolibrary.org/obo/GAZ_00005192"/>
        <obo:IAO_0000115>A large peninsula in northeastern New Britain, Papua New Guinea.</obo:IAO_0000115>
        <oboInOwl:hasOBONamespace>GAZ</oboInOwl:hasOBONamespace>
        <oboInOwl:id>GAZ:00053891</oboInOwl:id>
        <rdfs:label>Gazelle Peninsula</rdfs:label>
    </owl:NamedIndividual>
    


    <!-- http://purl.obolibrary.org/obo/GAZ_00053892 -->

    <owl:NamedIndividual rdf:about="http://purl.obolibrary.org/obo/GAZ_00053892">
        <obo:RO_0001025 rdf:resource="http://purl.obolibrary.org/obo/GAZ_00005189"/>
        <obo:RO_0001025 rdf:resource="http://purl.obolibrary.org/obo/GAZ_00005191"/>
        <obo:IAO_0000115>A volcano situated on the island of New Britain, Papua New Guinea, about 130 km southwest of Rabaul. A basaltic-to-andesitic stratovolcano it is the highest volcano of the Bismarck arc, and one of Papua New Guinea&apos;s most frequently active. Ulawun volcano, also known as the North Son, rises above the north coast of the island of New Britain across a low saddle NE of Bamus volcano, the South Son. The upper 1000 m of the 2334 m high Ulawun volcano is unvegetated. A prominent E-W-trending escarpment on the south may be the result of large-scale slumping. Satellitic cones occupy the NW and eastern flanks. A steep-walled valley cuts the NW side of Ulawun volcano, and a flank lava-flow complex lies to the south of this valley.</obo:IAO_0000115>
        <oboInOwl:hasOBONamespace>GAZ</oboInOwl:hasOBONamespace>
        <oboInOwl:id>GAZ:00053892</oboInOwl:id>
        <rdfs:label>Ulawun Volcano</rdfs:label>
    </owl:NamedIndividual>
    


    <!-- http://purl.obolibrary.org/obo/GAZ_00053893 -->

    <owl:NamedIndividual rdf:about="http://purl.obolibrary.org/obo/GAZ_00053893">
        <obo:RO_0001025 rdf:resource="http://purl.obolibrary.org/obo/GAZ_00005189"/>
        <obo:RO_0001025 rdf:resource="http://purl.obolibrary.org/obo/GAZ_00005191"/>
        <obo:IAO_0000115>A complex volcano that consists of a group of four small overlapping composite basaltic-andesitic cones on the lower eastern flank of the extinct Talawe volcano. Talawe is the highest volcano in the Cape Gloucester area of NW New Britain. A rectangular, 2.5 km-long crater is breached widely to the SE; Langila volcano was constructed NE of the breached crater of Talawe. An extensive lava field reaches the coast on the north and NE sides of Langila.</obo:IAO_0000115>
        <oboInOwl:hasOBONamespace>GAZ</oboInOwl:hasOBONamespace>
        <oboInOwl:id>GAZ:00053893</oboInOwl:id>
        <rdfs:label>Langila Volcano</rdfs:label>
    </owl:NamedIndividual>
    


    <!-- http://purl.obolibrary.org/obo/GAZ_00053894 -->

    <owl:NamedIndividual rdf:about="http://purl.obolibrary.org/obo/GAZ_00053894">
        <obo:RO_0001025 rdf:resource="http://purl.obolibrary.org/obo/GAZ_00005189"/>
        <obo:RO_0001025 rdf:resource="http://purl.obolibrary.org/obo/GAZ_00005191"/>
        <obo:IAO_0000115>A basaltic-to-dacitic volcano group consists of three volcanic peaks, Krummel, Garbuna, and Welcker. They are located along a 7 km N-S line above a shield-like foundation at the southern end of the Willaumez Peninsula. The central and lower peaks of the centrally located 564 m high Garbuna volcano contain a large vegetation-free area that is probably the most extensive thermal field in Papua New Guinea. A prominent lava dome and blocky lava flow in the center of thermal area have resisted destruction by thermal activity, and may be of Holocene age. The 854 m high Krummel volcano at the south end of the group contains a summit crater, breached to the NW. The highest peak of the Garbuna group is 1005 m high Welcker volcano, which has fed blocky lava flows that extend to the eastern coast of the peninsula.</obo:IAO_0000115>
        <oboInOwl:hasOBONamespace>GAZ</oboInOwl:hasOBONamespace>
        <oboInOwl:id>GAZ:00053894</oboInOwl:id>
        <rdfs:label>Garbuna Volcanic Group</rdfs:label>
    </owl:NamedIndividual>
    


    <!-- http://purl.obolibrary.org/obo/GAZ_00053895 -->

    <owl:NamedIndividual rdf:about="http://purl.obolibrary.org/obo/GAZ_00053895">
        <obo:RO_0001025 rdf:resource="http://purl.obolibrary.org/obo/GAZ_00053894"/>
        <oboInOwl:hasOBONamespace>GAZ</oboInOwl:hasOBONamespace>
        <oboInOwl:id>GAZ:00053895</oboInOwl:id>
        <rdfs:label>Krummel Volcano</rdfs:label>
    </owl:NamedIndividual>
    


    <!-- http://purl.obolibrary.org/obo/GAZ_00053896 -->

    <owl:NamedIndividual rdf:about="http://purl.obolibrary.org/obo/GAZ_00053896">
        <obo:RO_0001025 rdf:resource="http://purl.obolibrary.org/obo/GAZ_00053894"/>
        <oboInOwl:hasOBONamespace>GAZ</oboInOwl:hasOBONamespace>
        <oboInOwl:id>GAZ:00053896</oboInOwl:id>
        <rdfs:label>Welcker Volcano</rdfs:label>
    </owl:NamedIndividual>
    


    <!-- http://purl.obolibrary.org/obo/GAZ_00053897 -->

    <owl:NamedIndividual rdf:about="http://purl.obolibrary.org/obo/GAZ_00053897">
        <obo:RO_0001025 rdf:resource="http://purl.obolibrary.org/obo/GAZ_00053894"/>
        <oboInOwl:hasOBONamespace>GAZ</oboInOwl:hasOBONamespace>
        <oboInOwl:id>GAZ:00053897</oboInOwl:id>
        <rdfs:label>Garbuna Volcano</rdfs:label>
    </owl:NamedIndividual>
    


    <!-- http://purl.obolibrary.org/obo/GAZ_00053898 -->

    <owl:NamedIndividual rdf:about="http://purl.obolibrary.org/obo/GAZ_00053898">
        <obo:RO_0001025 rdf:resource="http://purl.obolibrary.org/obo/GAZ_00005189"/>
        <obo:RO_0001025 rdf:resource="http://purl.obolibrary.org/obo/GAZ_00005191"/>
        <obo:IAO_0000115>A group of overlapping small stratovolcanos on the island of New Britain in Papua New Guinea. The highest point in Mount Malopu at the southwestern end of the complex.</obo:IAO_0000115>
        <oboInOwl:hasOBONamespace>GAZ</oboInOwl:hasOBONamespace>
        <oboInOwl:id>GAZ:00053898</oboInOwl:id>
        <rdfs:label>Sulu Range</rdfs:label>
    </owl:NamedIndividual>
    


    <!-- http://purl.obolibrary.org/obo/GAZ_00053899 -->

    <owl:NamedIndividual rdf:about="http://purl.obolibrary.org/obo/GAZ_00053899">
        <obo:RO_0001025 rdf:resource="http://purl.obolibrary.org/obo/GAZ_00053898"/>
        <obo:IAO_0000115>The highest point of the Sulo Range.</obo:IAO_0000115>
        <oboInOwl:hasOBONamespace>GAZ</oboInOwl:hasOBONamespace>
        <oboInOwl:id>GAZ:00053899</oboInOwl:id>
        <rdfs:label>Mount Malopu</rdfs:label>
    </owl:NamedIndividual>
    


    <!-- http://purl.obolibrary.org/obo/GAZ_00053900 -->

    <owl:NamedIndividual rdf:about="http://purl.obolibrary.org/obo/GAZ_00053900">
        <obo:RO_0001025 rdf:resource="http://purl.obolibrary.org/obo/GAZ_00005189"/>
        <obo:RO_0001025 rdf:resource="http://purl.obolibrary.org/obo/GAZ_00022346"/>
        <obo:IAO_0000115>A large volcano situated in East New Britain, Papua New Guinea. A pyroclastic shield located on the tip of the Gazelle Peninsula at the NE end of New Britain. It forms a broad sheltered harbor utilized by what was the island&apos;s largest city prior to a major eruption in 1994. The outer flanks of the 688 m high asymmetrical pyroclastic shield volcano are formed by thick pyroclastic-flow deposits. The 8 x 14 km caldera is widely breached on the east, where its floor is flooded by Blanche Bay and was formed about 1400 years ago. An earlier caldera-forming eruption about 7100 years ago is now considered to have originated from Tavui caldera, offshore to the north. Three small stratovolcanoes lie outside the northern and NE caldera rims of Rabaul. Post-caldera eruptions built basaltic-to-dacitic pyroclastic cones on the caldera floor near the NE and western caldera walls. Several of these, including Vulcan cone, which was formed during a large eruption in 1878, have produced major explosive activity during historical time.</obo:IAO_0000115>
        <oboInOwl:hasOBONamespace>GAZ</oboInOwl:hasOBONamespace>
        <oboInOwl:id>GAZ:00053900</oboInOwl:id>
        <rdfs:label>Rabaul Caldera</rdfs:label>
    </owl:NamedIndividual>
    


    <!-- http://purl.obolibrary.org/obo/GAZ_00053901 -->

    <owl:NamedIndividual rdf:about="http://purl.obolibrary.org/obo/GAZ_00053901">
        <obo:RO_0001025 rdf:resource="http://purl.obolibrary.org/obo/GAZ_00053900"/>
        <obo:IAO_0000115>An active stratovolcano near Rabaul in East New Britain province, Papua New Guinea. It is a sub-vent of the Rabaul caldera and lies on the eastern rim of the larger feature.</obo:IAO_0000115>
        <oboInOwl:hasOBONamespace>GAZ</oboInOwl:hasOBONamespace>
        <oboInOwl:id>GAZ:00053901</oboInOwl:id>
        <rdfs:label>Tavurvur Volcano</rdfs:label>
    </owl:NamedIndividual>
    


    <!-- http://purl.obolibrary.org/obo/GAZ_00053902 -->

    <owl:NamedIndividual rdf:about="http://purl.obolibrary.org/obo/GAZ_00053902">
        <obo:RO_0001025 rdf:resource="http://purl.obolibrary.org/obo/GAZ_00053900"/>
        <obo:IAO_0000115>A pumice cone in Papua New Guinea. It is a sub-vent of the Rabaul caldera and lies on the western rim of the larger feature.</obo:IAO_0000115>
        <oboInOwl:hasOBONamespace>GAZ</oboInOwl:hasOBONamespace>
        <oboInOwl:id>GAZ:00053902</oboInOwl:id>
        <rdfs:label>Vulcan Volcano</rdfs:label>
    </owl:NamedIndividual>
    


    <!-- http://purl.obolibrary.org/obo/GAZ_00053903 -->

    <owl:NamedIndividual rdf:about="http://purl.obolibrary.org/obo/GAZ_00053903">
        <obo:RO_0001025 rdf:resource="http://purl.obolibrary.org/obo/GAZ_00016847"/>
        <obo:IAO_0000115>The northernmost of the Witu Islands, which lie north of western New Britain. Narage is the summit of a Pleistocene stratovolcano that displays strong thermal activity.</obo:IAO_0000115>
        <oboInOwl:hasOBONamespace>GAZ</oboInOwl:hasOBONamespace>
        <oboInOwl:id>GAZ:00053903</oboInOwl:id>
        <rdfs:label>Narage Island</rdfs:label>
    </owl:NamedIndividual>
    


    <!-- http://purl.obolibrary.org/obo/GAZ_00053904 -->

    <owl:NamedIndividual rdf:about="http://purl.obolibrary.org/obo/GAZ_00053904">
        <obo:RO_0001025 rdf:resource="http://purl.obolibrary.org/obo/GAZ_00016847"/>
        <obo:IAO_0000115>A small group of islands formed by a cluster of basaltic volcanoes. The largest volcanic center is formed by the western tip of the 7 km wide, linear Mundua Island and the arcuate Wingoru Island immediately to the west. The crater of this volcano is flooded by the sea through narrow channels on the northern and southern sides; remnants of crater walls form Wingoru island and are exposed at the western tip of Mundua island. Five small cones occupy the central and eastern sides of Mundua.</obo:IAO_0000115>
        <oboInOwl:hasOBONamespace>GAZ</oboInOwl:hasOBONamespace>
        <oboInOwl:id>GAZ:00053904</oboInOwl:id>
        <rdfs:label>Mundua Islands</rdfs:label>
    </owl:NamedIndividual>
    


    <!-- http://purl.obolibrary.org/obo/GAZ_00053905 -->

    <owl:NamedIndividual rdf:about="http://purl.obolibrary.org/obo/GAZ_00053905">
        <obo:RO_0001025 rdf:resource="http://purl.obolibrary.org/obo/GAZ_00053904"/>
        <obo:IAO_0000115>One of the Mundua Islands.</obo:IAO_0000115>
        <oboInOwl:hasOBONamespace>GAZ</oboInOwl:hasOBONamespace>
        <oboInOwl:id>GAZ:00053905</oboInOwl:id>
        <rdfs:label>Wingoru Island</rdfs:label>
    </owl:NamedIndividual>
    


    <!-- http://purl.obolibrary.org/obo/GAZ_00053906 -->

    <owl:NamedIndividual rdf:about="http://purl.obolibrary.org/obo/GAZ_00053906">
        <obo:RO_0001025 rdf:resource="http://purl.obolibrary.org/obo/GAZ_00053904"/>
        <obo:IAO_0000115>One of the Mundua Islands.</obo:IAO_0000115>
        <oboInOwl:hasOBONamespace>GAZ</oboInOwl:hasOBONamespace>
        <oboInOwl:id>GAZ:00053906</oboInOwl:id>
        <rdfs:label>Mundua Island</rdfs:label>
    </owl:NamedIndividual>
    


    <!-- http://purl.obolibrary.org/obo/GAZ_00053907 -->

    <owl:NamedIndividual rdf:about="http://purl.obolibrary.org/obo/GAZ_00053907">
        <obo:RO_0001025 rdf:resource="http://purl.obolibrary.org/obo/GAZ_00005189"/>
        <obo:RO_0001025 rdf:resource="http://purl.obolibrary.org/obo/GAZ_00005191"/>
        <obo:IAO_0000115>A peninsula. It runs N from the N coast of New Britain.</obo:IAO_0000115>
        <oboInOwl:hasOBONamespace>GAZ</oboInOwl:hasOBONamespace>
        <oboInOwl:id>GAZ:00053907</oboInOwl:id>
        <rdfs:label>Willaumez Peninsula</rdfs:label>
    </owl:NamedIndividual>
    


    <!-- http://purl.obolibrary.org/obo/GAZ_00053908 -->

    <owl:NamedIndividual rdf:about="http://purl.obolibrary.org/obo/GAZ_00053908">
        <obo:RO_0001025 rdf:resource="http://purl.obolibrary.org/obo/GAZ_00053907"/>
        <obo:IAO_0000115>A caldera anchoring the northern tip of the Willaumez Peninsula, is one of New Britain&apos;s most dramatic volcanoes. The latest episode of caldera formation occurred as recently as about 1150 years ago, and was followed by at least 5 subplinian or vulcanian eruptions. A 12 km wide, freshwater lake whose surface is only about 50 m above sea level occupies the caldera. Two vertical fault-bounded blocks form topographic highs at the western and eastern sides of the caldera. A N-S-trending line of post-caldera cones, explosion craters, and part of an arcuate inner caldera rim form a large peninsula that nearly bisects the horseshoe-shaped caldera lake.</obo:IAO_0000115>
        <oboInOwl:hasOBONamespace>GAZ</oboInOwl:hasOBONamespace>
        <oboInOwl:id>GAZ:00053908</oboInOwl:id>
        <rdfs:label>Dakataua Caldera</rdfs:label>
    </owl:NamedIndividual>
    


    <!-- http://purl.obolibrary.org/obo/GAZ_00053909 -->

    <owl:NamedIndividual rdf:about="http://purl.obolibrary.org/obo/GAZ_00053909">
        <obo:RO_0001025 rdf:resource="http://purl.obolibrary.org/obo/GAZ_00053907"/>
        <obo:IAO_0000115>A stratovolcano.</obo:IAO_0000115>
        <oboInOwl:hasOBONamespace>GAZ</oboInOwl:hasOBONamespace>
        <oboInOwl:id>GAZ:00053909</oboInOwl:id>
        <rdfs:label>Mount Makalia</rdfs:label>
    </owl:NamedIndividual>
    


    <!-- http://purl.obolibrary.org/obo/GAZ_00053910 -->

    <owl:NamedIndividual rdf:about="http://purl.obolibrary.org/obo/GAZ_00053910">
        <obo:RO_0001025 rdf:resource="http://purl.obolibrary.org/obo/GAZ_00053907"/>
        <obo:IAO_0000115>A symmetrical stratovolcano, located immediately SW of Dakataua caldera, that forms the 1155-m high point of the Willaumez Peninsula. The forested andesitic cone has a well-preserved, 400-m-wide crater with a 100 m high eastern wall and a low western rim. Three large explosion craters occupy the NE flank of Bola. The most recent lava flow issued from the summit crater and flowed to the west. This viscous flow is at least 50 m thick, leaving an irregularity in the profile of the volcano.</obo:IAO_0000115>
        <oboInOwl:hasOBONamespace>GAZ</oboInOwl:hasOBONamespace>
        <oboInOwl:id>GAZ:00053910</oboInOwl:id>
        <rdfs:label>Bola Volcano</rdfs:label>
    </owl:NamedIndividual>
    


    <!-- http://purl.obolibrary.org/obo/GAZ_00053911 -->

    <owl:NamedIndividual rdf:about="http://purl.obolibrary.org/obo/GAZ_00053911">
        <obo:RO_0001025 rdf:resource="http://purl.obolibrary.org/obo/GAZ_00005189"/>
        <obo:RO_0001025 rdf:resource="http://purl.obolibrary.org/obo/GAZ_00005191"/>
        <obo:IAO_0000115>A volcanic field that consists of a group of lava domes and ash cones of possible Holocene age. These volcanic vents ring the harbor on the west and form Garua Island to the east. Much of the volcanic field, including the two lava domes on Garua Island, consists of rhyolitic rocks. Active hot springs ring the shores of Garua Harbour and are best developed on the north and south sides. Large boiling pools, fumaroles, and small geysers are found on the north shore near Pangalu village. Another large group of boiling pools, fumaroles, and mudpots is located near the Talasea Government Station on the south shore of the bay.</obo:IAO_0000115>
        <oboInOwl:hasOBONamespace>GAZ</oboInOwl:hasOBONamespace>
        <oboInOwl:id>GAZ:00053911</oboInOwl:id>
        <rdfs:label>Garua Harbour Volcanic Field</rdfs:label>
    </owl:NamedIndividual>
    


    <!-- http://purl.obolibrary.org/obo/GAZ_00053912 -->

    <owl:NamedIndividual rdf:about="http://purl.obolibrary.org/obo/GAZ_00053912">
        <obo:RO_0001025 rdf:resource="http://purl.obolibrary.org/obo/GAZ_00005189"/>
        <obo:IAO_0000115>A small, nearly symmetrical 805 m high andesitic stratovolcano located north of Pago volcano along the north coast of New Britain near Cape Hoskins.</obo:IAO_0000115>
        <oboInOwl:hasOBONamespace>GAZ</oboInOwl:hasOBONamespace>
        <oboInOwl:id>GAZ:00053912</oboInOwl:id>
        <rdfs:label>Lolo Volcano</rdfs:label>
    </owl:NamedIndividual>
    


    <!-- http://purl.obolibrary.org/obo/GAZ_00053913 -->

    <owl:NamedIndividual rdf:about="http://purl.obolibrary.org/obo/GAZ_00053913">
        <obo:RO_0001025 rdf:resource="http://purl.obolibrary.org/obo/GAZ_00005189"/>
        <obo:RO_0001025 rdf:resource="http://purl.obolibrary.org/obo/GAZ_00005191"/>
        <oboInOwl:hasOBONamespace>GAZ</oboInOwl:hasOBONamespace>
        <oboInOwl:id>GAZ:00053913</oboInOwl:id>
        <rdfs:label>Witori Caldera</rdfs:label>
    </owl:NamedIndividual>
    


    <!-- http://purl.obolibrary.org/obo/GAZ_00053914 -->

    <owl:NamedIndividual rdf:about="http://purl.obolibrary.org/obo/GAZ_00053914">
        <obo:RO_0001025 rdf:resource="http://purl.obolibrary.org/obo/GAZ_00053913"/>
        <obo:IAO_0000115>A young post-caldera cone that was constructed within the 5.5 x 7.5 km Witori caldera. The Buru caldera cuts the SW flank of Witori volcano. The gently sloping outer flanks of Witori volcano consist primarily of dacitic pyroclastic-flow and airfall deposits produced during a series of five major explosive eruptions from about 5600 to 1200 years ago, many of which may have been assocciated with caldera formation. The post-caldera cone of Witori, Mount Pago, may have formed less than 350 years ago. Pago has grown to a height above that of the Witori caldera rim. A series of ten dacitic lava flows from Pago covers much of the caldera floor. The youngest of these was erupted during 2002-2003 from vents extending from the summit nearly to the NW caldera wall.</obo:IAO_0000115>
        <oboInOwl:hasOBONamespace>GAZ</oboInOwl:hasOBONamespace>
        <oboInOwl:id>GAZ:00053914</oboInOwl:id>
        <rdfs:label>Mount Pago</rdfs:label>
    </owl:NamedIndividual>
    


    <!-- http://purl.obolibrary.org/obo/GAZ_00053915 -->

    <owl:NamedIndividual rdf:about="http://purl.obolibrary.org/obo/GAZ_00053915">
        <obo:RO_0001025 rdf:resource="http://purl.obolibrary.org/obo/GAZ_00005189"/>
        <obo:IAO_0000115>A caldera, whose floor is 150 m above sea level, and which contains an inner caldera with a steep west-facing wall. A caldera lake on the SE side drains through a narrow gap in the northern caldera wall. The latest caldera-forming eruption of Hargy volcano took place about 11,000 years ago. The dacitic Galloseulo lava cone rises above and partially overtops the western rim of the caldera. A double crater occupies a larger 700-m-wide crater.</obo:IAO_0000115>
        <oboInOwl:hasOBONamespace>GAZ</oboInOwl:hasOBONamespace>
        <oboInOwl:id>GAZ:00053915</oboInOwl:id>
        <rdfs:label>Hargy Volcano</rdfs:label>
    </owl:NamedIndividual>
    


    <!-- http://purl.obolibrary.org/obo/GAZ_00053916 -->

    <owl:NamedIndividual rdf:about="http://purl.obolibrary.org/obo/GAZ_00053916">
        <obo:RO_0001025 rdf:resource="http://purl.obolibrary.org/obo/GAZ_00053915"/>
        <obo:IAO_0000115>A lava cone in the Hargy Caldera.</obo:IAO_0000115>
        <oboInOwl:hasOBONamespace>GAZ</oboInOwl:hasOBONamespace>
        <oboInOwl:id>GAZ:00053916</oboInOwl:id>
        <rdfs:label>Galloseulo Lava Cone</rdfs:label>
    </owl:NamedIndividual>
    


    <!-- http://purl.obolibrary.org/obo/GAZ_00053917 -->

    <owl:NamedIndividual rdf:about="http://purl.obolibrary.org/obo/GAZ_00053917">
        <obo:RO_0001025 rdf:resource="http://purl.obolibrary.org/obo/GAZ_00005189"/>
        <obo:RO_0001025 rdf:resource="http://purl.obolibrary.org/obo/GAZ_00005191"/>
        <obo:IAO_0000115>An andesitic stratovolcano is draped by rainforest and contains a breached summit crater filled with a lava dome. A satellitic cone is located on the southern flank, and a prominent 1.5 km wide crater with two small adjacent cones is situated halfway up the SE flank. Young pyroclastic-flow deposits are found on the volcano&apos;s flanks, and villagers describe an eruption that took place during the late-19th century.</obo:IAO_0000115>
        <oboInOwl:hasOBONamespace>GAZ</oboInOwl:hasOBONamespace>
        <oboInOwl:id>GAZ:00053917</oboInOwl:id>
        <rdfs:label>Bamus Volcano</rdfs:label>
    </owl:NamedIndividual>
    


    <!-- http://purl.obolibrary.org/obo/GAZ_00053918 -->

    <owl:NamedIndividual rdf:about="http://purl.obolibrary.org/obo/GAZ_00053918">
        <rdf:type rdf:resource="http://purl.obolibrary.org/obo/ENVO_00000222"/>
        <obo:RO_0001025 rdf:resource="http://purl.obolibrary.org/obo/GAZ_00005193"/>
        <obo:IAO_0000115>A volcanic island off the E coast of New Britain.</obo:IAO_0000115>
        <oboInOwl:hasOBONamespace>GAZ</oboInOwl:hasOBONamespace>
        <oboInOwl:id>GAZ:00053918</oboInOwl:id>
        <rdfs:label>Lolobau Island</rdfs:label>
    </owl:NamedIndividual>
    


    <!-- http://purl.obolibrary.org/obo/GAZ_00053919 -->

    <owl:NamedIndividual rdf:about="http://purl.obolibrary.org/obo/GAZ_00053919">
        <obo:RO_0001025 rdf:resource="http://purl.obolibrary.org/obo/GAZ_00053918"/>
        <obo:IAO_0000115>A small lake occupies the SW part of the caldera. A small lava dome (Hulu) caps Mount Lolobau, which has a 0.8 x 1.1 km summit crater that is breached to the NE. Flank cones are found along the coast of the largely submerged volcano. Several vents within the caldera along an E-W-trending line on the eastern flank of Mount Lolobau have been active during historical time.</obo:IAO_0000115>
        <oboInOwl:hasOBONamespace>GAZ</oboInOwl:hasOBONamespace>
        <oboInOwl:id>GAZ:00053919</oboInOwl:id>
        <rdfs:label>Mount Lolobau</rdfs:label>
    </owl:NamedIndividual>
    


    <!-- http://purl.obolibrary.org/obo/GAZ_00053920 -->

    <owl:NamedIndividual rdf:about="http://purl.obolibrary.org/obo/GAZ_00053920">
        <obo:RO_0001025 rdf:resource="http://purl.obolibrary.org/obo/GAZ_00005189"/>
        <obo:RO_0001025 rdf:resource="http://purl.obolibrary.org/obo/GAZ_00005192"/>
        <obo:IAO_0000115>A mostly submarine caldera that lies off the NE tip of the Gazelle Peninsula north of Rabaul caldera. The caldera was first discovered during a bathymetric cruise in 1985. The SW wall of the roughly 10 x 12 km wide Tavui caldera cuts the NE tip of the peninsula and extends from Tavui Point at the northern tip of the peninsula SE to Laweo Point. The 7100-year-old Raluan Ignimbrite, initially thought to have originated from Rabaul caldera, is now thought to have been produced by an eruption of Tavui caldera. A basaltic scoria layer immediately underlies the rhyolitic ignimbrite, and the introduction of basaltic magma was considered to have triggered the rhyolitic eruption.</obo:IAO_0000115>
        <oboInOwl:hasOBONamespace>GAZ</oboInOwl:hasOBONamespace>
        <oboInOwl:id>GAZ:00053920</oboInOwl:id>
        <rdfs:label>Tavui Caldera</rdfs:label>
    </owl:NamedIndividual>
    


    <!-- http://purl.obolibrary.org/obo/GAZ_00053924 -->

    <owl:NamedIndividual rdf:about="http://purl.obolibrary.org/obo/GAZ_00053924">
        <obo:RO_0001025 rdf:resource="http://purl.obolibrary.org/obo/GAZ_00012664"/>
        <obo:IAO_0000115>A stratovolcano at the western end of a volcanic chain in the highlands of Papua New Guinea, rise to 3568 m and are dominated by two westward-facing escarpments of probable landslide origin. Satellite cones and lava domes occur on the NE and southern flanks of the dominantly andesitic volcano.</obo:IAO_0000115>
        <oboInOwl:hasOBONamespace>GAZ</oboInOwl:hasOBONamespace>
        <oboInOwl:id>GAZ:00053924</oboInOwl:id>
        <rdfs:label>Doma Peaks</rdfs:label>
    </owl:NamedIndividual>
    


    <!-- http://purl.obolibrary.org/obo/GAZ_00053926 -->

    <owl:NamedIndividual rdf:about="http://purl.obolibrary.org/obo/GAZ_00053926">
        <obo:RO_0001025 rdf:resource="http://purl.obolibrary.org/obo/GAZ_00003922"/>
        <obo:IAO_0000115>A stratovolcano that contains a group of andesitic lava domes in the summit area and NW flank. Marble Peak is an older volcanic center immediately to the south. The largest dome in the summit crater is perforated by at least 11 craters. Two large steep-sided, flat-topped lava domes occupy the NNE flank, and two smaller domes are located to the west.</obo:IAO_0000115>
        <oboInOwl:hasOBONamespace>GAZ</oboInOwl:hasOBONamespace>
        <oboInOwl:id>GAZ:00053926</oboInOwl:id>
        <rdfs:label>Mount Yelia</rdfs:label>
    </owl:NamedIndividual>
    


    <!-- http://purl.obolibrary.org/obo/GAZ_00053927 -->

    <owl:NamedIndividual rdf:about="http://purl.obolibrary.org/obo/GAZ_00053927">
        <obo:IAO_0000115>A Pliocene-to-Holocene hydrothermal explosion vent complex (Pigram et al., 1977), is located in the Morobe goldfields in the Owen Stanley Range SW of Huon Gulf.</obo:IAO_0000115>
        <oboInOwl:hasOBONamespace>GAZ</oboInOwl:hasOBONamespace>
        <oboInOwl:id>GAZ:00053927</oboInOwl:id>
        <rdfs:label>Koranga Crater</rdfs:label>
    </owl:NamedIndividual>
    


    <!-- http://purl.obolibrary.org/obo/GAZ_00053929 -->

    <owl:NamedIndividual rdf:about="http://purl.obolibrary.org/obo/GAZ_00053929">
        <obo:IAO_0000115>The highest point in the Owen Stanley Ranges in Central Province, Papua New Guinea at 4,072 m. It lies approximately 75 km north-north-west of Port Moresby.</obo:IAO_0000115>
        <oboInOwl:hasOBONamespace>GAZ</oboInOwl:hasOBONamespace>
        <oboInOwl:id>GAZ:00053929</oboInOwl:id>
        <rdfs:label>Mount Victoria</rdfs:label>
    </owl:NamedIndividual>
    


    <!-- http://purl.obolibrary.org/obo/GAZ_00053930 -->

    <owl:NamedIndividual rdf:about="http://purl.obolibrary.org/obo/GAZ_00053930">
        <obo:IAO_0000115>An isolated, well-preserved pyroclastic cone located on the SW side of the Owen Stanley Range about 50 km NE of Port Moresby. The small volcano, which was not recognized until 1969, rises about 250 m from the flood plain of the Naoro River. A lava flow extends 1 km to the west from the breached summit crater.</obo:IAO_0000115>
        <oboInOwl:hasOBONamespace>GAZ</oboInOwl:hasOBONamespace>
        <oboInOwl:id>GAZ:00053930</oboInOwl:id>
        <rdfs:label>Madilogo Volcano</rdfs:label>
    </owl:NamedIndividual>
    


    <!-- http://purl.obolibrary.org/obo/GAZ_00053931 -->

    <owl:NamedIndividual rdf:about="http://purl.obolibrary.org/obo/GAZ_00053931">
        <obo:RO_0001025 rdf:resource="http://purl.obolibrary.org/obo/GAZ_00012662"/>
        <obo:IAO_0000115>An andesitic stratovolcano in the Northern Province of Papua New Guinea. Mount Lamington rises to 1680 m above the coastal plain north of the Owen Stanley Range. A summit complex of lava domes and crater remnants rises above a low-angle base of volcaniclastic deposits that are dissected by radial valleys. A prominent broad &quot;avalanche valley&quot; extends northward from the breached crater. Ash layers from two early Holocene eruptions at Lamington have been identified. After a long quiescent period, the volcano sprang suddenly to life in 1951, producing a powerful explosive eruption during which devastating pyroclastic flows and surges swept all sides of the volcano, killing nearly 3000 persons. The eruption concluded with growth of a 560 m high lava dome in the summit crater.</obo:IAO_0000115>
        <oboInOwl:hasOBONamespace>GAZ</oboInOwl:hasOBONamespace>
        <oboInOwl:id>GAZ:00053931</oboInOwl:id>
        <rdfs:label>Mount Lamington</rdfs:label>
    </owl:NamedIndividual>
    


    <!-- http://purl.obolibrary.org/obo/GAZ_00053932 -->

    <owl:NamedIndividual rdf:about="http://purl.obolibrary.org/obo/GAZ_00053932">
        <obo:RO_0001025 rdf:resource="http://purl.obolibrary.org/obo/GAZ_00012662"/>
        <obo:IAO_0000115>A forested, deeply dissected andesitic volcanic massif extending from the eastern margin of Mount Lamington north to the coast of eastern Papua New Guinea.</obo:IAO_0000115>
        <oboInOwl:hasOBONamespace>GAZ</oboInOwl:hasOBONamespace>
        <oboInOwl:id>GAZ:00053932</oboInOwl:id>
        <rdfs:label>Hydrographers Range</rdfs:label>
    </owl:NamedIndividual>
    


    <!-- http://purl.obolibrary.org/obo/GAZ_00053933 -->

    <owl:NamedIndividual rdf:about="http://purl.obolibrary.org/obo/GAZ_00053933">
        <obo:RO_0001025 rdf:resource="http://purl.obolibrary.org/obo/GAZ_00012662"/>
        <obo:IAO_0000115>Hot springs and thermal vents at Musa River are located in metamorphic terrain with no obvious connection to recent volcanic activity. Basement rocks are metamorphic schists, and Tertiary andesitic volcanics are found less than 1 km away.</obo:IAO_0000115>
        <oboInOwl:hasOBONamespace>GAZ</oboInOwl:hasOBONamespace>
        <oboInOwl:id>GAZ:00053933</oboInOwl:id>
        <rdfs:label>Musa River Hydrothermal Field</rdfs:label>
    </owl:NamedIndividual>
    


    <!-- http://purl.obolibrary.org/obo/GAZ_00053934 -->

    <owl:NamedIndividual rdf:about="http://purl.obolibrary.org/obo/GAZ_00053934">
        <obo:RO_0001025 rdf:resource="http://purl.obolibrary.org/obo/GAZ_00003922"/>
        <obo:IAO_0000115>A volcanic field with thirty small volcanic centers of late-Pleistocene to Holocene age, located in SE Papua New Guinea on the Managlase Plateau, south of the Hydrographers Range and SW of the Dyke Ackland Bay. The fault-bounded plateau forms a triangular-shaped area dotted with trachybasaltic lava cones and flows, scoria mounds, cinder cones, and explosion vents of the Uoivi Volcanics and capped on its eastern side by rhyodacitic ash cones, lava domes, and ashflow deposits of the Manna Volcanics.</obo:IAO_0000115>
        <oboInOwl:hasOBONamespace>GAZ</oboInOwl:hasOBONamespace>
        <oboInOwl:id>GAZ:00053934</oboInOwl:id>
        <rdfs:label>Managlase Plateau Volcanic Field</rdfs:label>
    </owl:NamedIndividual>
    


    <!-- http://purl.obolibrary.org/obo/GAZ_00053935 -->

    <owl:NamedIndividual rdf:about="http://purl.obolibrary.org/obo/GAZ_00053935">
        <rdf:type rdf:resource="http://purl.obolibrary.org/obo/ENVO_00000305"/>
        <obo:RO_0001025 rdf:resource="http://purl.obolibrary.org/obo/GAZ_00012662"/>
        <obo:IAO_0000115>A cape.</obo:IAO_0000115>
        <oboInOwl:hasOBONamespace>GAZ</oboInOwl:hasOBONamespace>
        <oboInOwl:id>GAZ:00053935</oboInOwl:id>
        <rdfs:label>Cape Nelson</rdfs:label>
    </owl:NamedIndividual>
    


    <!-- http://purl.obolibrary.org/obo/GAZ_00053936 -->

    <owl:NamedIndividual rdf:about="http://purl.obolibrary.org/obo/GAZ_00053936">
        <obo:RO_0001025 rdf:resource="http://purl.obolibrary.org/obo/GAZ_00053935"/>
        <obo:IAO_0000115>A stratovolcano on the NE coast of Papua New Guinea. Mount Victory is densely mantled by rainforest, which is somewhat stunted near the summit. On the NE it abutts the deeply dissected Pleistocene Mount Trafalgar volcano. The summit crater of Mount Victory is breached to the SE and is of possible landslide origin. Several near-summit lava domes are present, the SE-most of which marks the 1925 m high summit of the volcano. Four small satellite cones are located on the SW side, and two others occur on the NE flank.</obo:IAO_0000115>
        <oboInOwl:hasOBONamespace>GAZ</oboInOwl:hasOBONamespace>
        <oboInOwl:id>GAZ:00053936</oboInOwl:id>
        <rdfs:label>Mount Victory</rdfs:label>
    </owl:NamedIndividual>
    


    <!-- http://purl.obolibrary.org/obo/GAZ_00053937 -->

    <owl:NamedIndividual rdf:about="http://purl.obolibrary.org/obo/GAZ_00053937">
        <obo:RO_0001025 rdf:resource="http://purl.obolibrary.org/obo/GAZ_00003922"/>
        <obo:IAO_0000115>Pyroclastic cones located near the mouth of the Uiaka River, south of Collingwood Bay. A small alkalic andesitic volcanic field in eastern Papua New Guinea.</obo:IAO_0000115>
        <oboInOwl:hasOBONamespace>GAZ</oboInOwl:hasOBONamespace>
        <oboInOwl:id>GAZ:00053937</oboInOwl:id>
        <rdfs:label>Sessagara Hills</rdfs:label>
    </owl:NamedIndividual>
    


    <!-- http://purl.obolibrary.org/obo/GAZ_00053938 -->

    <owl:NamedIndividual rdf:about="http://purl.obolibrary.org/obo/GAZ_00053938">
        <obo:RO_0001025 rdf:resource="http://purl.obolibrary.org/obo/GAZ_00003922"/>
        <obo:IAO_0000115>An isolated pyroclastic cone that was formed during 1943-44 by explosive eruptions through Paleozoic to pre-Cambrian metamorphic rocks.</obo:IAO_0000115>
        <oboInOwl:hasOBONamespace>GAZ</oboInOwl:hasOBONamespace>
        <oboInOwl:id>GAZ:00053938</oboInOwl:id>
        <rdfs:label>Waiowa Volcano</rdfs:label>
    </owl:NamedIndividual>
    


    <!-- http://purl.obolibrary.org/obo/GAZ_00053939 -->

    <owl:NamedIndividual rdf:about="http://purl.obolibrary.org/obo/GAZ_00053939">
        <obo:RO_0001025 rdf:resource="http://purl.obolibrary.org/obo/GAZ_00016854"/>
        <obo:IAO_0000115>A roughly circular volcanic island that is the westernmost of the D&apos;Entrecasteaux Islands off the NE tip of Papua New Guinea. Several basaltic-andesite and andesitic Holocene eruptive centers that may be only a few hundred years old are located around the margins of fault-bounded metamorphic rocks that form the central part of Goodenough Island. The youngest volcanic features, which include the Walilagi Cones, are located at the SE end of the island. These well-developed ash cones and blocky lava flows on the northern and eastern flanks of the Bwaido Peninsula may have erupted within the past few hundred years.</obo:IAO_0000115>
        <oboInOwl:hasOBONamespace>GAZ</oboInOwl:hasOBONamespace>
        <oboInOwl:id>GAZ:00053939</oboInOwl:id>
        <rdfs:label>Goodenough Island Volcanic Field</rdfs:label>
    </owl:NamedIndividual>
    


    <!-- http://purl.obolibrary.org/obo/GAZ_00053940 -->

    <owl:NamedIndividual rdf:about="http://purl.obolibrary.org/obo/GAZ_00053940">
        <obo:RO_0001025 rdf:resource="http://purl.obolibrary.org/obo/GAZ_00016854"/>
        <obo:IAO_0000115>A protected area. Established 1981.</obo:IAO_0000115>
        <oboInOwl:hasOBONamespace>GAZ</oboInOwl:hasOBONamespace>
        <oboInOwl:id>GAZ:00053940</oboInOwl:id>
        <rdfs:label>Oi Mada Wara Wildlife Management Area</rdfs:label>
    </owl:NamedIndividual>
    


    <!-- http://purl.obolibrary.org/obo/GAZ_00053941 -->

    <owl:NamedIndividual rdf:about="http://purl.obolibrary.org/obo/GAZ_00053941">
        <obo:RO_0001025 rdf:resource="http://purl.obolibrary.org/obo/GAZ_00016855"/>
        <obo:IAO_0000115>An area of youthful volcanism and active thermal fields is located on the SW part of Fergusson Island, in the center of the D&apos;Entrecasteaux island group. The Iamalele-Fagululu area contains a series of lava domes and lava flows of probable Holocene age in association with abundant hot springs and fumaroles (Smith 1981). Two small lava domes are located near Fagululu village, the largest of which is a 150 m high flat-topped, obsidian-bearing rhyolitic dome. Six other lava domes are clustered around Salt Lake on the western side of the area. Hot springs, boiling springs, fumaroles, and mud pools are found in an area of siliceous sinter near Iamalele village.</obo:IAO_0000115>
        <oboInOwl:hasOBONamespace>GAZ</oboInOwl:hasOBONamespace>
        <oboInOwl:id>GAZ:00053941</oboInOwl:id>
        <rdfs:label>Iamalele Lava Domes</rdfs:label>
    </owl:NamedIndividual>
    


    <!-- http://purl.obolibrary.org/obo/GAZ_00053942 -->

    <owl:NamedIndividual rdf:about="http://purl.obolibrary.org/obo/GAZ_00053942">
        <obo:RO_0001025 rdf:resource="http://purl.obolibrary.org/obo/GAZ_00016854"/>
        <obo:IAO_0000115>The highest peak in the D&apos;Entrecasteaux Islands.</obo:IAO_0000115>
        <oboInOwl:hasOBONamespace>GAZ</oboInOwl:hasOBONamespace>
        <oboInOwl:id>GAZ:00053942</oboInOwl:id>
        <rdfs:label>Mount Vineuo</rdfs:label>
    </owl:NamedIndividual>
    


    <!-- http://purl.obolibrary.org/obo/GAZ_00053943 -->

    <owl:NamedIndividual rdf:about="http://purl.obolibrary.org/obo/GAZ_00053943">
        <obo:RO_0001025 rdf:resource="http://purl.obolibrary.org/obo/GAZ_00007181"/>
        <obo:IAO_0000115>A volcanic field in the Dawson Straits with several volcanic centers that define a possible partly submerged caldera. There have been no historical eruptions from this center, but morphology suggests an extremely young age for some lava flows, and the area displays vigorous thermal activity. The most prominent volcanic centers are Mounts Lamonai and Oiau, located about 10 km apart on the SW tip of Fergusson Island. The 500 m high summit of Lamonai is capped by a steep-walled crater, and rhyolitic lava flows are exposed on the NE side of the cone. Dominantly volcaniclastic Oiau cone has also produced obsidian lava flows. Dobu Island to the south is formed of coalescing volcanic centers and likewise has produced youthful rhyolitic obsidian flows.</obo:IAO_0000115>
        <oboInOwl:hasOBONamespace>GAZ</oboInOwl:hasOBONamespace>
        <oboInOwl:id>GAZ:00053943</oboInOwl:id>
        <rdfs:label>Dawson Strait Volcanic Field</rdfs:label>
    </owl:NamedIndividual>
    


    <!-- http://purl.obolibrary.org/obo/GAZ_00053944 -->

    <owl:NamedIndividual rdf:about="http://purl.obolibrary.org/obo/GAZ_00053944">
        <obo:RO_0001025 rdf:resource="http://purl.obolibrary.org/obo/GAZ_00005188"/>
        <obo:IAO_0000115>The highest peak of New Ireland.</obo:IAO_0000115>
        <oboInOwl:hasOBONamespace>GAZ</oboInOwl:hasOBONamespace>
        <oboInOwl:id>GAZ:00053944</oboInOwl:id>
        <rdfs:label>Mount Lambel</rdfs:label>
    </owl:NamedIndividual>
    


    <!-- http://purl.obolibrary.org/obo/GAZ_00053945 -->

    <owl:NamedIndividual rdf:about="http://purl.obolibrary.org/obo/GAZ_00053945">
        <obo:RO_0001025 rdf:resource="http://purl.obolibrary.org/obo/GAZ_00012664"/>
        <obo:IAO_0000115>The second highest mountain in Papua New Guinea at 4,368 m. It is located in the Southern Highlands province and is an old shield volcano with vast alpine grasslands. Ancient volcanic plugs form its two summits, with the central peak the highest and an east peak about 2 km away at 4,300 m.</obo:IAO_0000115>
        <oboInOwl:hasOBONamespace>GAZ</oboInOwl:hasOBONamespace>
        <oboInOwl:id>GAZ:00053945</oboInOwl:id>
        <rdfs:label>Mount Giluwe</rdfs:label>
    </owl:NamedIndividual>
    


    <!-- http://purl.obolibrary.org/obo/GAZ_00053946 -->

    <owl:NamedIndividual rdf:about="http://purl.obolibrary.org/obo/GAZ_00053946">
        <obo:RO_0001025 rdf:resource="http://purl.obolibrary.org/obo/GAZ_00012660"/>
        <obo:RO_0001025 rdf:resource="http://purl.obolibrary.org/obo/GAZ_00012661"/>
        <obo:IAO_0000115>An eroded stratovolcano located on the border between the Western Highlands and Enga Provinces, about 24 km NW of the city of Mount Hagen which is named after it.</obo:IAO_0000115>
        <oboInOwl:hasOBONamespace>GAZ</oboInOwl:hasOBONamespace>
        <oboInOwl:id>GAZ:00053946</oboInOwl:id>
        <rdfs:label>Mount Hagen</rdfs:label>
    </owl:NamedIndividual>
    


    <!-- http://purl.obolibrary.org/obo/GAZ_00053947 -->

    <owl:NamedIndividual rdf:about="http://purl.obolibrary.org/obo/GAZ_00053947">
        <obo:RO_0001025 rdf:resource="http://purl.obolibrary.org/obo/GAZ_00005184"/>
        <obo:IAO_0000115>A mountain range in northern part of the island of Bougainville, Papua New Guinea. Several volcanoes are located in the range, including highest point of the island - Mount Balbi.</obo:IAO_0000115>
        <oboInOwl:hasOBONamespace>GAZ</oboInOwl:hasOBONamespace>
        <oboInOwl:id>GAZ:00053947</oboInOwl:id>
        <rdfs:label>Emperor Range</rdfs:label>
    </owl:NamedIndividual>
    


    <!-- http://purl.obolibrary.org/obo/GAZ_00053948 -->

    <owl:NamedIndividual rdf:about="http://purl.obolibrary.org/obo/GAZ_00053948">
        <obo:RO_0001025 rdf:resource="http://purl.obolibrary.org/obo/GAZ_00053947"/>
        <obo:IAO_0000115>A caldera the southern and SW sides of pf whose rim are covered by lava flows that extend up to 14 km from a large post-caldera lava cone. The summit of the andesitic volcano consists of an erosional pyramidal peak and a forested satellitic ash cone 3 km to the NW.</obo:IAO_0000115>
        <oboInOwl:hasOBONamespace>GAZ</oboInOwl:hasOBONamespace>
        <oboInOwl:id>GAZ:00053948</oboInOwl:id>
        <rdfs:label>Tore Volcano</rdfs:label>
    </owl:NamedIndividual>
    


    <!-- http://purl.obolibrary.org/obo/GAZ_00053949 -->

    <owl:NamedIndividual rdf:about="http://purl.obolibrary.org/obo/GAZ_00053949">
        <obo:RO_0001025 rdf:resource="http://purl.obolibrary.org/obo/GAZ_00053947"/>
        <obo:IAO_0000115>A stratovolcano located in the northern portion of the island of Bougainville, Papua New Guinea. It is the highest point of the island. There are five volcanic craters along a ridge north of the summit, one of which contains a crater lake. There are numerous fumaroles near the craters.</obo:IAO_0000115>
        <oboInOwl:hasOBONamespace>GAZ</oboInOwl:hasOBONamespace>
        <oboInOwl:id>GAZ:00053949</oboInOwl:id>
        <rdfs:label>Mount Balbi</rdfs:label>
    </owl:NamedIndividual>
    


    <!-- http://purl.obolibrary.org/obo/GAZ_00053950 -->

    <owl:NamedIndividual rdf:about="http://purl.obolibrary.org/obo/GAZ_00053950">
        <obo:RO_0001025 rdf:resource="http://purl.obolibrary.org/obo/GAZ_00053947"/>
        <obo:IAO_0000115>A small pyroclastic shield immediately NE of Bagana volcano, has produced some of the largest Holocene eruptions of Papua New Guinea. Andesitic-to-dacitic Billy Mitchell volcano is truncated by a 2 km wide caldera containing a shallow lake with a small island near its southern shore. Two major explosive eruptions, one about 900 years ago and the other about 370 years ago, produced dacitic pyroclastic-fall deposits that cover most of the northern half of Bougainville Island. The younger eruption may have been responsible for formation of the nearly vertical, steep-walled summit caldera. Pyroclastic-flow and -surge deposits from Billy Mitchell extend 25 km to the eastern coast of Bougainville Island.</obo:IAO_0000115>
        <oboInOwl:hasOBONamespace>GAZ</oboInOwl:hasOBONamespace>
        <oboInOwl:id>GAZ:00053950</oboInOwl:id>
        <rdfs:label>Billy Mitchell Volcano</rdfs:label>
    </owl:NamedIndividual>
    


    <!-- http://purl.obolibrary.org/obo/GAZ_00053951 -->

    <owl:NamedIndividual rdf:about="http://purl.obolibrary.org/obo/GAZ_00053951">
        <obo:RO_0001025 rdf:resource="http://purl.obolibrary.org/obo/GAZ_00053947"/>
        <obo:IAO_0000115>A massive symmetrical, roughly 1750 m high lava cone largely constructed by an accumulation of viscous andesitic lava flows. The entire lava cone could have been constructed in about 300 years at its present rate of lava production. Eruptive activity at Bagana is frequent and is characterized by non-explosive effusion of viscous lava that maintains a small lava dome in the summit crater, although explosive activity occasionally producing pyroclastic flows also occurs. Lava flows form dramatic, freshly preserved tongue-shaped lobes up to 50-m-thick with prominent levees that descend the volcano&apos;s flanks on all sides.</obo:IAO_0000115>
        <oboInOwl:hasOBONamespace>GAZ</oboInOwl:hasOBONamespace>
        <oboInOwl:id>GAZ:00053951</oboInOwl:id>
        <rdfs:label>Bagana Volcano</rdfs:label>
    </owl:NamedIndividual>
    


    <!-- http://purl.obolibrary.org/obo/GAZ_00053952 -->

    <owl:NamedIndividual rdf:about="http://purl.obolibrary.org/obo/GAZ_00053952">
        <rdf:type rdf:resource="http://purl.obolibrary.org/obo/ENVO_00000354"/>
        <obo:RO_0001025 rdf:resource="http://purl.obolibrary.org/obo/GAZ_00005184"/>
        <obo:IAO_0000115>A volcanic complex that consists of three closely spaced, NW-SE-trending andesitic-dacitic stratovolcanoes. Two of these are relatively uneroded and have probably been active during the Holocene, and a third, extensively eroded volcano is probably Pleistocene in age (Blake and Meizitis 1967). Along with Loloru volcano, the Takuan volcanoes are post-caldera cones constructed along the rim of the Pleistocene Laluai caldera. The 2210-m NW-most volcano, Mount Takuan, is the highest of the group and is a lava cone that has fed viscous lavas flows to the south, similar to those at Bagana volcano. The central volcano contains a large lava dome in its breached summit crater; this dome may represent the most recent activity of the Takuan volcano group. Older, but still well-preserved lava flows are found on the flanks of this volcano.</obo:IAO_0000115>
        <oboInOwl:hasOBONamespace>GAZ</oboInOwl:hasOBONamespace>
        <oboInOwl:id>GAZ:00053952</oboInOwl:id>
        <rdfs:label>Takuan Volcanic Complex</rdfs:label>
    </owl:NamedIndividual>
    


    <!-- http://purl.obolibrary.org/obo/GAZ_00053953 -->

    <owl:NamedIndividual rdf:about="http://purl.obolibrary.org/obo/GAZ_00053953">
        <obo:RO_0001025 rdf:resource="http://purl.obolibrary.org/obo/GAZ_00053952"/>
        <oboInOwl:hasOBONamespace>GAZ</oboInOwl:hasOBONamespace>
        <oboInOwl:id>GAZ:00053953</oboInOwl:id>
        <rdfs:label>Mount Takuan</rdfs:label>
    </owl:NamedIndividual>
    


    <!-- http://purl.obolibrary.org/obo/GAZ_00053954 -->

    <owl:NamedIndividual rdf:about="http://purl.obolibrary.org/obo/GAZ_00053954">
        <obo:RO_0001025 rdf:resource="http://purl.obolibrary.org/obo/GAZ_00005184"/>
        <obo:IAO_0000115>A pyroclastic shield vulcano whose summit consists of two nested calderas, and a forested andesitic lava dome that restricts a crescent-shaped lake to the eastern side of the younger caldera. The smooth flanks of the pyroclastic shield are dissected by radiating deep valleys. A pristine lava flow occurs on the SE flank. Loloru is constructed within the 10 x 15 km Pleistocene Laluai caldera. The topographically higher Taroka group of volcanoes to the NW and the Takuan group to the north also were constructed within the caldera and served to deflect the bulk of Loloru ignimbrites to the south.</obo:IAO_0000115>
        <oboInOwl:hasOBONamespace>GAZ</oboInOwl:hasOBONamespace>
        <oboInOwl:id>GAZ:00053954</oboInOwl:id>
        <rdfs:label>Loloru Volcano</rdfs:label>
    </owl:NamedIndividual>
    


    <!-- http://purl.obolibrary.org/obo/GAZ_00056643 -->

    <owl:NamedIndividual rdf:about="http://purl.obolibrary.org/obo/GAZ_00056643">
        <obo:RO_0001025 rdf:resource="http://purl.obolibrary.org/obo/GAZ_00012658"/>
        <obo:IAO_0000115>A mountain range in the central highlands of Papua New Guinea. The Ramu River has its source in the range.</obo:IAO_0000115>
        <oboInOwl:hasOBONamespace>GAZ</oboInOwl:hasOBONamespace>
        <oboInOwl:id>GAZ:00056643</oboInOwl:id>
        <rdfs:label>Bismarck Range</rdfs:label>
    </owl:NamedIndividual>
    


    <!-- http://purl.obolibrary.org/obo/GAZ_00056645 -->

    <owl:NamedIndividual rdf:about="http://purl.obolibrary.org/obo/GAZ_00056645">
        <obo:RO_0001025 rdf:resource="http://purl.obolibrary.org/obo/GAZ_00012665"/>
        <obo:IAO_0000115>A mountain range in western Papua New Guinea, stretching from the Star Mountains to the east.</obo:IAO_0000115>
        <oboInOwl:hasOBONamespace>GAZ</oboInOwl:hasOBONamespace>
        <oboInOwl:id>GAZ:00056645</oboInOwl:id>
        <rdfs:label>Hindenburg Range</rdfs:label>
    </owl:NamedIndividual>
    


    <!-- http://purl.obolibrary.org/obo/GAZ_00057558 -->

    <owl:NamedIndividual rdf:about="http://purl.obolibrary.org/obo/GAZ_00057558">
        <obo:RO_0001025 rdf:resource="http://purl.obolibrary.org/obo/GAZ_00012665"/>
        <obo:IAO_0000115>A lake.</obo:IAO_0000115>
        <oboInOwl:hasOBONamespace>GAZ</oboInOwl:hasOBONamespace>
        <oboInOwl:id>GAZ:00057558</oboInOwl:id>
        <rdfs:label>Lake Daviumbu</rdfs:label>
    </owl:NamedIndividual>
    


    <!-- http://purl.obolibrary.org/obo/GAZ_00058479 -->

    <owl:NamedIndividual rdf:about="http://purl.obolibrary.org/obo/GAZ_00058479">
        <obo:RO_0001025 rdf:resource="http://purl.obolibrary.org/obo/GAZ_00003922"/>
        <obo:IAO_0000115>A mountain range.</obo:IAO_0000115>
        <oboInOwl:hasOBONamespace>GAZ</oboInOwl:hasOBONamespace>
        <oboInOwl:id>GAZ:00058479</oboInOwl:id>
        <rdfs:label>Victor Emanuel Range</rdfs:label>
    </owl:NamedIndividual>
    


    <!-- http://purl.obolibrary.org/obo/GAZ_00058480 -->

    <owl:NamedIndividual rdf:about="http://purl.obolibrary.org/obo/GAZ_00058480">
        <obo:RO_0001025 rdf:resource="http://purl.obolibrary.org/obo/GAZ_00012663"/>
        <obo:IAO_0000115>A mountain range in northwestern Papua New Guinea.</obo:IAO_0000115>
        <oboInOwl:hasOBONamespace>GAZ</oboInOwl:hasOBONamespace>
        <oboInOwl:id>GAZ:00058480</oboInOwl:id>
        <rdfs:label>Bewani Mountains</rdfs:label>
    </owl:NamedIndividual>
    


    <!-- http://purl.obolibrary.org/obo/GAZ_00058481 -->

    <owl:NamedIndividual rdf:about="http://purl.obolibrary.org/obo/GAZ_00058481">
        <obo:RO_0001025 rdf:resource="http://purl.obolibrary.org/obo/GAZ_00012663"/>
        <obo:IAO_0000115>A mountain range in Sandaun Province, northwestern Papua New Guinea. The Bewani Mountains are located to the west, and the Prince Alexander Mountains are located to the east. To the north, the mountains slope down to the Pacific Ocean, and to the south lies the basin of the Sepik River.</obo:IAO_0000115>
        <oboInOwl:hasOBONamespace>GAZ</oboInOwl:hasOBONamespace>
        <oboInOwl:id>GAZ:00058481</oboInOwl:id>
        <rdfs:label>Torricelli Mountains</rdfs:label>
    </owl:NamedIndividual>
    


    <!-- http://purl.obolibrary.org/obo/GAZ_00058482 -->

    <owl:NamedIndividual rdf:about="http://purl.obolibrary.org/obo/GAZ_00058482">
        <obo:RO_0001025 rdf:resource="http://purl.obolibrary.org/obo/GAZ_00003922"/>
        <obo:IAO_0000115>A mountain range in Papua New Guinea. The range is located on the northern coast of New Guinea. The Torricelli Mountains lie to the west, and the basin of the Sepik River lies to the south.</obo:IAO_0000115>
        <oboInOwl:hasOBONamespace>GAZ</oboInOwl:hasOBONamespace>
        <oboInOwl:id>GAZ:00058482</oboInOwl:id>
        <rdfs:label>Prince Alexander Mountains</rdfs:label>
    </owl:NamedIndividual>
    


    <!-- http://purl.obolibrary.org/obo/GAZ_00058483 -->

    <owl:NamedIndividual rdf:about="http://purl.obolibrary.org/obo/GAZ_00058483">
        <obo:RO_0001025 rdf:resource="http://purl.obolibrary.org/obo/GAZ_00005266"/>
        <obo:IAO_0000115>A series of swamps and canals that are seasonally filled by the flooding of the Sepik River in Papua New Guinea. The Chambri Lakes from in the middle Sepik, between the town of Pagwi and the junction of the Yuat River with the Sepik.</obo:IAO_0000115>
        <oboInOwl:hasOBONamespace>GAZ</oboInOwl:hasOBONamespace>
        <oboInOwl:id>GAZ:00058483</oboInOwl:id>
        <rdfs:label>Chambri Lakes</rdfs:label>
    </owl:NamedIndividual>
    


    <!-- http://purl.obolibrary.org/obo/GAZ_00058484 -->

    <owl:NamedIndividual rdf:about="http://purl.obolibrary.org/obo/GAZ_00058484">
        <obo:RO_0001025 rdf:resource="http://purl.obolibrary.org/obo/GAZ_00253980"/>
        <obo:IAO_0000115>A freshwater lake in the Southern Highlands province of Papua New Guinea. It lies to the east of the Kikori River, into which it eventually drains. It is about 50 km southwest of Mendi, the provincial capital. A Ramsar Site.</obo:IAO_0000115>
        <oboInOwl:hasOBONamespace>GAZ</oboInOwl:hasOBONamespace>
        <oboInOwl:id>GAZ:00058484</oboInOwl:id>
        <rdfs:label>Lake Kutubu</rdfs:label>
    </owl:NamedIndividual>
    


    <!-- http://purl.obolibrary.org/obo/GAZ_00058485 -->

    <owl:NamedIndividual rdf:about="http://purl.obolibrary.org/obo/GAZ_00058485">
        <obo:RO_0001025 rdf:resource="http://purl.obolibrary.org/obo/GAZ_00022419"/>
        <obo:RO_0001025 rdf:resource="http://purl.obolibrary.org/obo/GAZ_00253651"/>
        <obo:IAO_0000115>A lake in the Western Province of Papua New Guinea. It lies in a shallow depression between the Strickland and Fly Rivers. It is a lateral lake, formed by the blocking of a tributary of the Srickland River.</obo:IAO_0000115>
        <oboInOwl:hasOBONamespace>GAZ</oboInOwl:hasOBONamespace>
        <oboInOwl:id>GAZ:00058485</oboInOwl:id>
        <rdfs:label>Lake Murray</rdfs:label>
    </owl:NamedIndividual>
    


    <!-- http://purl.obolibrary.org/obo/GAZ_00117917 -->

    <owl:NamedIndividual rdf:about="http://purl.obolibrary.org/obo/GAZ_00117917">
        <obo:RO_0001025 rdf:resource="http://purl.obolibrary.org/obo/GAZ_00003922"/>
    </owl:NamedIndividual>
    


    <!-- http://purl.obolibrary.org/obo/GAZ_00117918 -->

    <owl:NamedIndividual rdf:about="http://purl.obolibrary.org/obo/GAZ_00117918"/>
    


    <!-- http://purl.obolibrary.org/obo/GAZ_00117919 -->

    <owl:NamedIndividual rdf:about="http://purl.obolibrary.org/obo/GAZ_00117919"/>
    


    <!-- http://purl.obolibrary.org/obo/GAZ_00117920 -->

    <owl:NamedIndividual rdf:about="http://purl.obolibrary.org/obo/GAZ_00117920"/>
    


    <!-- http://purl.obolibrary.org/obo/GAZ_00117921 -->

    <owl:NamedIndividual rdf:about="http://purl.obolibrary.org/obo/GAZ_00117921"/>
    


    <!-- http://purl.obolibrary.org/obo/GAZ_00117922 -->

    <owl:NamedIndividual rdf:about="http://purl.obolibrary.org/obo/GAZ_00117922">
        <obo:RO_0001025 rdf:resource="http://purl.obolibrary.org/obo/GAZ_00022388"/>
        <obo:IAO_0000115>A Local-Level Government Area of Bulolo District.</obo:IAO_0000115>
        <oboInOwl:hasOBONamespace>GAZ</oboInOwl:hasOBONamespace>
        <oboInOwl:id>GAZ:00117922</oboInOwl:id>
        <rdfs:label>Mumeng Rural Local-Level Government Area</rdfs:label>
    </owl:NamedIndividual>
    


    <!-- http://purl.obolibrary.org/obo/GAZ_00117923 -->

    <owl:NamedIndividual rdf:about="http://purl.obolibrary.org/obo/GAZ_00117923">
        <obo:RO_0001025 rdf:resource="http://purl.obolibrary.org/obo/GAZ_00022388"/>
        <obo:IAO_0000115>A Local-Level Government Area of Bulolo District.</obo:IAO_0000115>
        <oboInOwl:hasOBONamespace>GAZ</oboInOwl:hasOBONamespace>
        <oboInOwl:id>GAZ:00117923</oboInOwl:id>
        <rdfs:label>Watut Rural Local-Level Government Area</rdfs:label>
    </owl:NamedIndividual>
    


    <!-- http://purl.obolibrary.org/obo/GAZ_00117924 -->

    <owl:NamedIndividual rdf:about="http://purl.obolibrary.org/obo/GAZ_00117924">
        <obo:RO_0001025 rdf:resource="http://purl.obolibrary.org/obo/GAZ_00022388"/>
        <obo:IAO_0000115>A Local-Level Government Area of Bulolo District.</obo:IAO_0000115>
        <oboInOwl:hasOBONamespace>GAZ</oboInOwl:hasOBONamespace>
        <oboInOwl:id>GAZ:00117924</oboInOwl:id>
        <rdfs:label>Wau Rural Local-Level Government Area</rdfs:label>
    </owl:NamedIndividual>
    


    <!-- http://purl.obolibrary.org/obo/GAZ_00117925 -->

    <owl:NamedIndividual rdf:about="http://purl.obolibrary.org/obo/GAZ_00117925">
        <obo:RO_0001025 rdf:resource="http://purl.obolibrary.org/obo/GAZ_00022388"/>
        <obo:IAO_0000115>A Local-Level Government Area of Bulolo District.</obo:IAO_0000115>
        <oboInOwl:hasOBONamespace>GAZ</oboInOwl:hasOBONamespace>
        <oboInOwl:id>GAZ:00117925</oboInOwl:id>
        <rdfs:label>Wau-Bulolo Urban Local-Level Government Area</rdfs:label>
    </owl:NamedIndividual>
    


    <!-- http://purl.obolibrary.org/obo/GAZ_00117926 -->

    <owl:NamedIndividual rdf:about="http://purl.obolibrary.org/obo/GAZ_00117926">
        <obo:RO_0001025 rdf:resource="http://purl.obolibrary.org/obo/GAZ_00022388"/>
        <obo:IAO_0000115>A Local-Level Government Area of Bulolo District.</obo:IAO_0000115>
        <oboInOwl:hasOBONamespace>GAZ</oboInOwl:hasOBONamespace>
        <oboInOwl:id>GAZ:00117926</oboInOwl:id>
        <rdfs:label>Waria Rural Local-Level Government Area</rdfs:label>
    </owl:NamedIndividual>
    


    <!-- http://purl.obolibrary.org/obo/GAZ_00117927 -->

    <owl:NamedIndividual rdf:about="http://purl.obolibrary.org/obo/GAZ_00117927">
        <obo:RO_0001025 rdf:resource="http://purl.obolibrary.org/obo/GAZ_00022393"/>
        <obo:IAO_0000115>A Local-Level Government Area of Huon District.</obo:IAO_0000115>
        <oboInOwl:hasOBONamespace>GAZ</oboInOwl:hasOBONamespace>
        <oboInOwl:id>GAZ:00117927</oboInOwl:id>
        <rdfs:label>Morobe Rural Local-Level Government Area</rdfs:label>
    </owl:NamedIndividual>
    


    <!-- http://purl.obolibrary.org/obo/GAZ_00117928 -->

    <owl:NamedIndividual rdf:about="http://purl.obolibrary.org/obo/GAZ_00117928">
        <obo:RO_0001025 rdf:resource="http://purl.obolibrary.org/obo/GAZ_00022393"/>
        <obo:IAO_0000115>A Local-Level Government Area of Huon District.</obo:IAO_0000115>
        <oboInOwl:hasOBONamespace>GAZ</oboInOwl:hasOBONamespace>
        <oboInOwl:id>GAZ:00117928</oboInOwl:id>
        <rdfs:label>Salamaua Rural Local-Level Government Area</rdfs:label>
    </owl:NamedIndividual>
    


    <!-- http://purl.obolibrary.org/obo/GAZ_00117929 -->

    <owl:NamedIndividual rdf:about="http://purl.obolibrary.org/obo/GAZ_00117929">
        <obo:RO_0001025 rdf:resource="http://purl.obolibrary.org/obo/GAZ_00022393"/>
        <obo:IAO_0000115>A Local-Level Government Area of Huon District.</obo:IAO_0000115>
        <oboInOwl:hasOBONamespace>GAZ</oboInOwl:hasOBONamespace>
        <oboInOwl:id>GAZ:00117929</oboInOwl:id>
        <rdfs:label>Wampar Rural Local-Level Government Area</rdfs:label>
    </owl:NamedIndividual>
    


    <!-- http://purl.obolibrary.org/obo/GAZ_00117930 -->

    <owl:NamedIndividual rdf:about="http://purl.obolibrary.org/obo/GAZ_00117930">
        <obo:RO_0001025 rdf:resource="http://purl.obolibrary.org/obo/GAZ_00022390"/>
        <obo:IAO_0000115>A Local-Level Government Area of Kabwum District.</obo:IAO_0000115>
        <oboInOwl:hasOBONamespace>GAZ</oboInOwl:hasOBONamespace>
        <oboInOwl:id>GAZ:00117930</oboInOwl:id>
        <rdfs:label>Deyamos Rural Local-Level Government Area</rdfs:label>
    </owl:NamedIndividual>
    


    <!-- http://purl.obolibrary.org/obo/GAZ_00117931 -->

    <owl:NamedIndividual rdf:about="http://purl.obolibrary.org/obo/GAZ_00117931">
        <obo:RO_0001025 rdf:resource="http://purl.obolibrary.org/obo/GAZ_00022390"/>
        <obo:IAO_0000115>A Local-Level Government Area of Kabwum District.</obo:IAO_0000115>
        <oboInOwl:hasOBONamespace>GAZ</oboInOwl:hasOBONamespace>
        <oboInOwl:id>GAZ:00117931</oboInOwl:id>
        <rdfs:label>Seko Rural Local-Level Government Area</rdfs:label>
    </owl:NamedIndividual>
    


    <!-- http://purl.obolibrary.org/obo/GAZ_00117932 -->

    <owl:NamedIndividual rdf:about="http://purl.obolibrary.org/obo/GAZ_00117932">
        <obo:RO_0001025 rdf:resource="http://purl.obolibrary.org/obo/GAZ_00022390"/>
        <obo:IAO_0000115>A Local-Level Government Area of Kabwum District.</obo:IAO_0000115>
        <oboInOwl:hasOBONamespace>GAZ</oboInOwl:hasOBONamespace>
        <oboInOwl:id>GAZ:00117932</oboInOwl:id>
        <rdfs:label>Yus Rural Local-Level Government Area</rdfs:label>
    </owl:NamedIndividual>
    


    <!-- http://purl.obolibrary.org/obo/GAZ_00117933 -->

    <owl:NamedIndividual rdf:about="http://purl.obolibrary.org/obo/GAZ_00117933">
        <obo:RO_0001025 rdf:resource="http://purl.obolibrary.org/obo/GAZ_00022392"/>
        <obo:IAO_0000115>A Local-Level Government Area of Lae District.</obo:IAO_0000115>
        <oboInOwl:hasOBONamespace>GAZ</oboInOwl:hasOBONamespace>
        <oboInOwl:id>GAZ:00117933</oboInOwl:id>
        <rdfs:label>Ahi Rural Local-Level Government Area</rdfs:label>
    </owl:NamedIndividual>
    


    <!-- http://purl.obolibrary.org/obo/GAZ_00117934 -->

    <owl:NamedIndividual rdf:about="http://purl.obolibrary.org/obo/GAZ_00117934">
        <obo:RO_0001025 rdf:resource="http://purl.obolibrary.org/obo/GAZ_00022392"/>
        <obo:IAO_0000115>A Local-Level Government Area of Lae District.</obo:IAO_0000115>
        <oboInOwl:hasOBONamespace>GAZ</oboInOwl:hasOBONamespace>
        <oboInOwl:id>GAZ:00117934</oboInOwl:id>
        <rdfs:label>Lae Urban Local-Level Government Area</rdfs:label>
    </owl:NamedIndividual>
    


    <!-- http://purl.obolibrary.org/obo/GAZ_00117935 -->

    <owl:NamedIndividual rdf:about="http://purl.obolibrary.org/obo/GAZ_00117935">
        <obo:RO_0001025 rdf:resource="http://purl.obolibrary.org/obo/GAZ_00022395"/>
        <obo:IAO_0000115>A Local-Level Government Area of Markham District.</obo:IAO_0000115>
        <oboInOwl:hasOBONamespace>GAZ</oboInOwl:hasOBONamespace>
        <oboInOwl:id>GAZ:00117935</oboInOwl:id>
        <rdfs:label>Onga-Waffa Rural Local-Level Government Area</rdfs:label>
    </owl:NamedIndividual>
    


    <!-- http://purl.obolibrary.org/obo/GAZ_00117936 -->

    <owl:NamedIndividual rdf:about="http://purl.obolibrary.org/obo/GAZ_00117936">
        <obo:RO_0001025 rdf:resource="http://purl.obolibrary.org/obo/GAZ_00022395"/>
        <obo:IAO_0000115>A Local-Level Government Area of Markham District.</obo:IAO_0000115>
        <oboInOwl:hasOBONamespace>GAZ</oboInOwl:hasOBONamespace>
        <oboInOwl:id>GAZ:00117936</oboInOwl:id>
        <rdfs:label>Umi-Atzero Rural Local-Level Government Area</rdfs:label>
    </owl:NamedIndividual>
    


    <!-- http://purl.obolibrary.org/obo/GAZ_00117937 -->

    <owl:NamedIndividual rdf:about="http://purl.obolibrary.org/obo/GAZ_00117937">
        <obo:RO_0001025 rdf:resource="http://purl.obolibrary.org/obo/GAZ_00022395"/>
        <obo:IAO_0000115>A Local-Level Government Area of Markham District.</obo:IAO_0000115>
        <oboInOwl:hasOBONamespace>GAZ</oboInOwl:hasOBONamespace>
        <oboInOwl:id>GAZ:00117937</oboInOwl:id>
        <rdfs:label>Wantoat-Leron Rural Local-Level Government Area</rdfs:label>
    </owl:NamedIndividual>
    


    <!-- http://purl.obolibrary.org/obo/GAZ_00117938 -->

    <owl:NamedIndividual rdf:about="http://purl.obolibrary.org/obo/GAZ_00117938">
        <obo:RO_0001025 rdf:resource="http://purl.obolibrary.org/obo/GAZ_00022391"/>
        <obo:IAO_0000115>A Local-Level Government Area of Menyamya District.</obo:IAO_0000115>
        <oboInOwl:hasOBONamespace>GAZ</oboInOwl:hasOBONamespace>
        <oboInOwl:id>GAZ:00117938</oboInOwl:id>
        <rdfs:label>Aseki Rural Local-Level Government Area</rdfs:label>
    </owl:NamedIndividual>
    


    <!-- http://purl.obolibrary.org/obo/GAZ_00117939 -->

    <owl:NamedIndividual rdf:about="http://purl.obolibrary.org/obo/GAZ_00117939">
        <obo:RO_0001025 rdf:resource="http://purl.obolibrary.org/obo/GAZ_00022391"/>
        <obo:IAO_0000115>A Local-Level Government Area of Menyamya District.</obo:IAO_0000115>
        <oboInOwl:hasOBONamespace>GAZ</oboInOwl:hasOBONamespace>
        <oboInOwl:id>GAZ:00117939</oboInOwl:id>
        <rdfs:label>Wapi Rural Local-Level Government Area</rdfs:label>
    </owl:NamedIndividual>
    


    <!-- http://purl.obolibrary.org/obo/GAZ_00117940 -->

    <owl:NamedIndividual rdf:about="http://purl.obolibrary.org/obo/GAZ_00117940">
        <obo:RO_0001025 rdf:resource="http://purl.obolibrary.org/obo/GAZ_00022391"/>
        <obo:IAO_0000115>A Local-Level Government Area of Menyamya District.</obo:IAO_0000115>
        <oboInOwl:hasOBONamespace>GAZ</oboInOwl:hasOBONamespace>
        <oboInOwl:id>GAZ:00117940</oboInOwl:id>
        <rdfs:label>Kome Rural Local-Level Government Area</rdfs:label>
    </owl:NamedIndividual>
    


    <!-- http://purl.obolibrary.org/obo/GAZ_00117941 -->

    <owl:NamedIndividual rdf:about="http://purl.obolibrary.org/obo/GAZ_00117941">
        <obo:RO_0001025 rdf:resource="http://purl.obolibrary.org/obo/GAZ_00022394"/>
        <obo:IAO_0000115>A Local-Level Government Area of Nawae District.</obo:IAO_0000115>
        <oboInOwl:hasOBONamespace>GAZ</oboInOwl:hasOBONamespace>
        <oboInOwl:id>GAZ:00117941</oboInOwl:id>
        <rdfs:label>Labuta Rural Local-Level Government Area</rdfs:label>
    </owl:NamedIndividual>
    


    <!-- http://purl.obolibrary.org/obo/GAZ_00117942 -->

    <owl:NamedIndividual rdf:about="http://purl.obolibrary.org/obo/GAZ_00117942">
        <obo:RO_0001025 rdf:resource="http://purl.obolibrary.org/obo/GAZ_00022394"/>
        <obo:IAO_0000115>A Local-Level Government Area of Nawae District.</obo:IAO_0000115>
        <oboInOwl:hasOBONamespace>GAZ</oboInOwl:hasOBONamespace>
        <oboInOwl:id>GAZ:00117942</oboInOwl:id>
        <rdfs:label>Nabak Rural Local-Level Government Area</rdfs:label>
    </owl:NamedIndividual>
    


    <!-- http://purl.obolibrary.org/obo/GAZ_00117943 -->

    <owl:NamedIndividual rdf:about="http://purl.obolibrary.org/obo/GAZ_00117943">
        <obo:RO_0001025 rdf:resource="http://purl.obolibrary.org/obo/GAZ_00022394"/>
        <obo:IAO_0000115>A Local-Level Government Area of Nawae District.</obo:IAO_0000115>
        <oboInOwl:hasOBONamespace>GAZ</oboInOwl:hasOBONamespace>
        <oboInOwl:id>GAZ:00117943</oboInOwl:id>
        <rdfs:label>Wain-Erap Rural Local-Level Government Area</rdfs:label>
    </owl:NamedIndividual>
    


    <!-- http://purl.obolibrary.org/obo/GAZ_00117945 -->

    <owl:NamedIndividual rdf:about="http://purl.obolibrary.org/obo/GAZ_00117945">
        <obo:RO_0001025 rdf:resource="http://purl.obolibrary.org/obo/GAZ_00022389"/>
        <obo:IAO_0000115>A Local-Level Government Area of Tewae District.</obo:IAO_0000115>
        <oboInOwl:hasOBONamespace>GAZ</oboInOwl:hasOBONamespace>
        <oboInOwl:id>GAZ:00117945</oboInOwl:id>
        <rdfs:label>Sialum Rural Local-Level Government Area</rdfs:label>
    </owl:NamedIndividual>
    


    <!-- http://purl.obolibrary.org/obo/GAZ_00117946 -->

    <owl:NamedIndividual rdf:about="http://purl.obolibrary.org/obo/GAZ_00117946">
        <obo:RO_0001025 rdf:resource="http://purl.obolibrary.org/obo/GAZ_00022389"/>
        <obo:IAO_0000115>A Local-Level Government Area of Tewae District.</obo:IAO_0000115>
        <oboInOwl:hasOBONamespace>GAZ</oboInOwl:hasOBONamespace>
        <oboInOwl:id>GAZ:00117946</oboInOwl:id>
        <rdfs:label>Siassi Rural Local-Level Government Area</rdfs:label>
    </owl:NamedIndividual>
    


    <!-- http://purl.obolibrary.org/obo/GAZ_00117947 -->

    <owl:NamedIndividual rdf:about="http://purl.obolibrary.org/obo/GAZ_00117947">
        <obo:RO_0001025 rdf:resource="http://purl.obolibrary.org/obo/GAZ_00022389"/>
        <obo:IAO_0000115>A Local-Level Government Area of Tewae District.</obo:IAO_0000115>
        <oboInOwl:hasOBONamespace>GAZ</oboInOwl:hasOBONamespace>
        <oboInOwl:id>GAZ:00117947</oboInOwl:id>
        <rdfs:label>Wasu Rural Local-Level Government Area</rdfs:label>
    </owl:NamedIndividual>
    


    <!-- http://purl.obolibrary.org/obo/GAZ_00117948 -->

    <owl:NamedIndividual rdf:about="http://purl.obolibrary.org/obo/GAZ_00117948">
        <obo:RO_0001025 rdf:resource="http://purl.obolibrary.org/obo/GAZ_00005198"/>
        <obo:IAO_0000115>An island.</obo:IAO_0000115>
        <oboInOwl:hasOBONamespace>GAZ</oboInOwl:hasOBONamespace>
        <oboInOwl:id>GAZ:00117948</oboInOwl:id>
        <rdfs:label>Bagabag Island</rdfs:label>
    </owl:NamedIndividual>
    


    <!-- http://purl.obolibrary.org/obo/GAZ_00117949 -->

    <owl:NamedIndividual rdf:about="http://purl.obolibrary.org/obo/GAZ_00117949">
        <obo:RO_0001025 rdf:resource="http://purl.obolibrary.org/obo/GAZ_00022361"/>
        <obo:IAO_0000115>A Local-Level Government Area of Bogia District.</obo:IAO_0000115>
        <oboInOwl:hasOBONamespace>GAZ</oboInOwl:hasOBONamespace>
        <oboInOwl:id>GAZ:00117949</oboInOwl:id>
        <rdfs:label>Almami Rural Local-Level Government Area</rdfs:label>
    </owl:NamedIndividual>
    


    <!-- http://purl.obolibrary.org/obo/GAZ_00117950 -->

    <owl:NamedIndividual rdf:about="http://purl.obolibrary.org/obo/GAZ_00117950">
        <obo:RO_0001025 rdf:resource="http://purl.obolibrary.org/obo/GAZ_00022361"/>
        <obo:IAO_0000115>A Local-Level Government Area of Bogia District.</obo:IAO_0000115>
        <oboInOwl:hasOBONamespace>GAZ</oboInOwl:hasOBONamespace>
        <oboInOwl:id>GAZ:00117950</oboInOwl:id>
        <rdfs:label>Iabu Rural Local-Level Government Area</rdfs:label>
    </owl:NamedIndividual>
    


    <!-- http://purl.obolibrary.org/obo/GAZ_00117951 -->

    <owl:NamedIndividual rdf:about="http://purl.obolibrary.org/obo/GAZ_00117951">
        <obo:RO_0001025 rdf:resource="http://purl.obolibrary.org/obo/GAZ_00022361"/>
        <obo:IAO_0000115>A Local-Level Government Area of Bogia District.</obo:IAO_0000115>
        <oboInOwl:hasOBONamespace>GAZ</oboInOwl:hasOBONamespace>
        <oboInOwl:id>GAZ:00117951</oboInOwl:id>
        <rdfs:label>Yawar Rural Local-Level Government Area</rdfs:label>
    </owl:NamedIndividual>
    


    <!-- http://purl.obolibrary.org/obo/GAZ_00117952 -->

    <owl:NamedIndividual rdf:about="http://purl.obolibrary.org/obo/GAZ_00117952">
        <obo:RO_0001025 rdf:resource="http://purl.obolibrary.org/obo/GAZ_00022365"/>
        <obo:IAO_0000115>A Local-Level Government Area of Madang District.</obo:IAO_0000115>
        <oboInOwl:hasOBONamespace>GAZ</oboInOwl:hasOBONamespace>
        <oboInOwl:id>GAZ:00117952</oboInOwl:id>
        <rdfs:label>Ambenob Rural Local-Level Government Area</rdfs:label>
    </owl:NamedIndividual>
    


    <!-- http://purl.obolibrary.org/obo/GAZ_00117953 -->

    <owl:NamedIndividual rdf:about="http://purl.obolibrary.org/obo/GAZ_00117953">
        <obo:RO_0001025 rdf:resource="http://purl.obolibrary.org/obo/GAZ_00022365"/>
        <obo:IAO_0000115>A Local-Level Government Area of Madang District.</obo:IAO_0000115>
        <oboInOwl:hasOBONamespace>GAZ</oboInOwl:hasOBONamespace>
        <oboInOwl:id>GAZ:00117953</oboInOwl:id>
        <rdfs:label>Madang Urban Local-Level Government Area</rdfs:label>
    </owl:NamedIndividual>
    


    <!-- http://purl.obolibrary.org/obo/GAZ_00117954 -->

    <owl:NamedIndividual rdf:about="http://purl.obolibrary.org/obo/GAZ_00117954">
        <obo:RO_0001025 rdf:resource="http://purl.obolibrary.org/obo/GAZ_00022365"/>
        <obo:IAO_0000115>A Local-Level Government Area of Madang District.</obo:IAO_0000115>
        <oboInOwl:hasOBONamespace>GAZ</oboInOwl:hasOBONamespace>
        <oboInOwl:id>GAZ:00117954</oboInOwl:id>
        <rdfs:label>Transgogol Rural Local-Level Government Area</rdfs:label>
    </owl:NamedIndividual>
    


    <!-- http://purl.obolibrary.org/obo/GAZ_00117955 -->

    <owl:NamedIndividual rdf:about="http://purl.obolibrary.org/obo/GAZ_00117955">
        <obo:RO_0001025 rdf:resource="http://purl.obolibrary.org/obo/GAZ_00022366"/>
        <obo:IAO_0000115>A Local-Level Government Area of Middle Ramu District.</obo:IAO_0000115>
        <oboInOwl:hasOBONamespace>GAZ</oboInOwl:hasOBONamespace>
        <oboInOwl:id>GAZ:00117955</oboInOwl:id>
        <rdfs:label>Arabaka Rural Local-Level Government Area</rdfs:label>
    </owl:NamedIndividual>
    


    <!-- http://purl.obolibrary.org/obo/GAZ_00117956 -->

    <owl:NamedIndividual rdf:about="http://purl.obolibrary.org/obo/GAZ_00117956">
        <obo:RO_0001025 rdf:resource="http://purl.obolibrary.org/obo/GAZ_00022366"/>
        <obo:IAO_0000115>A Local-Level Government Area of Middle Ramu District.</obo:IAO_0000115>
        <oboInOwl:hasOBONamespace>GAZ</oboInOwl:hasOBONamespace>
        <oboInOwl:id>GAZ:00117956</oboInOwl:id>
        <rdfs:label>Josephstaal Rural Local-Level Government Area</rdfs:label>
    </owl:NamedIndividual>
    


    <!-- http://purl.obolibrary.org/obo/GAZ_00117957 -->

    <owl:NamedIndividual rdf:about="http://purl.obolibrary.org/obo/GAZ_00117957">
        <obo:RO_0001025 rdf:resource="http://purl.obolibrary.org/obo/GAZ_00022366"/>
        <obo:IAO_0000115>A Local-Level Government Area of Middle Ramu District.</obo:IAO_0000115>
        <oboInOwl:hasOBONamespace>GAZ</oboInOwl:hasOBONamespace>
        <oboInOwl:id>GAZ:00117957</oboInOwl:id>
        <rdfs:label>Simbai Rural Local-Level Government Area</rdfs:label>
    </owl:NamedIndividual>
    


    <!-- http://purl.obolibrary.org/obo/GAZ_00117958 -->

    <owl:NamedIndividual rdf:about="http://purl.obolibrary.org/obo/GAZ_00117958">
        <obo:RO_0001025 rdf:resource="http://purl.obolibrary.org/obo/GAZ_00022364"/>
        <obo:IAO_0000115>A Local-Level Government Area of Rai Coast District.</obo:IAO_0000115>
        <oboInOwl:hasOBONamespace>GAZ</oboInOwl:hasOBONamespace>
        <oboInOwl:id>GAZ:00117958</oboInOwl:id>
        <rdfs:label>Astrolabe Bay Rural Local-Level Government Area</rdfs:label>
    </owl:NamedIndividual>
    


    <!-- http://purl.obolibrary.org/obo/GAZ_00117959 -->

    <owl:NamedIndividual rdf:about="http://purl.obolibrary.org/obo/GAZ_00117959">
        <obo:RO_0001025 rdf:resource="http://purl.obolibrary.org/obo/GAZ_00022364"/>
        <obo:IAO_0000115>A Local-Level Government Area of Rai Coast District.</obo:IAO_0000115>
        <oboInOwl:hasOBONamespace>GAZ</oboInOwl:hasOBONamespace>
        <oboInOwl:id>GAZ:00117959</oboInOwl:id>
        <rdfs:label>Naho Rawa Rural Local-Level Government Area</rdfs:label>
    </owl:NamedIndividual>
    


    <!-- http://purl.obolibrary.org/obo/GAZ_00117960 -->

    <owl:NamedIndividual rdf:about="http://purl.obolibrary.org/obo/GAZ_00117960">
        <obo:RO_0001025 rdf:resource="http://purl.obolibrary.org/obo/GAZ_00022364"/>
        <obo:IAO_0000115>A Local-Level Government Area of Rai Coast District.</obo:IAO_0000115>
        <oboInOwl:hasOBONamespace>GAZ</oboInOwl:hasOBONamespace>
        <oboInOwl:id>GAZ:00117960</oboInOwl:id>
        <rdfs:label>Saidor Rural Local-Level Government Area</rdfs:label>
    </owl:NamedIndividual>
    


    <!-- http://purl.obolibrary.org/obo/GAZ_00117961 -->

    <owl:NamedIndividual rdf:about="http://purl.obolibrary.org/obo/GAZ_00117961">
        <obo:RO_0001025 rdf:resource="http://purl.obolibrary.org/obo/GAZ_00022362"/>
        <obo:IAO_0000115>A Local-Level Government Area of Sumkar District.</obo:IAO_0000115>
        <oboInOwl:hasOBONamespace>GAZ</oboInOwl:hasOBONamespace>
        <oboInOwl:id>GAZ:00117961</oboInOwl:id>
        <rdfs:label>Sumgilbar Rural Local-Level Government Area</rdfs:label>
    </owl:NamedIndividual>
    


    <!-- http://purl.obolibrary.org/obo/GAZ_00117962 -->

    <owl:NamedIndividual rdf:about="http://purl.obolibrary.org/obo/GAZ_00117962">
        <obo:RO_0001025 rdf:resource="http://purl.obolibrary.org/obo/GAZ_00022362"/>
        <obo:IAO_0000115>A Local-Level Government Area of Sumkar District.</obo:IAO_0000115>
        <oboInOwl:hasOBONamespace>GAZ</oboInOwl:hasOBONamespace>
        <oboInOwl:id>GAZ:00117962</oboInOwl:id>
        <rdfs:label>Karkar Rural Local-Level Government Area</rdfs:label>
    </owl:NamedIndividual>
    


    <!-- http://purl.obolibrary.org/obo/GAZ_00117963 -->

    <owl:NamedIndividual rdf:about="http://purl.obolibrary.org/obo/GAZ_00117963">
        <obo:RO_0001025 rdf:resource="http://purl.obolibrary.org/obo/GAZ_00022363"/>
        <obo:IAO_0000115>A Local-Level Government Area of Usino Bundi District.</obo:IAO_0000115>
        <oboInOwl:hasOBONamespace>GAZ</oboInOwl:hasOBONamespace>
        <oboInOwl:id>GAZ:00117963</oboInOwl:id>
        <rdfs:label>Bundi Rural Local-Level Government Area</rdfs:label>
    </owl:NamedIndividual>
    


    <!-- http://purl.obolibrary.org/obo/GAZ_00117964 -->

    <owl:NamedIndividual rdf:about="http://purl.obolibrary.org/obo/GAZ_00117964">
        <obo:RO_0001025 rdf:resource="http://purl.obolibrary.org/obo/GAZ_00022363"/>
        <obo:IAO_0000115>A Local-Level Government Area of Usino Bundi District.</obo:IAO_0000115>
        <oboInOwl:hasOBONamespace>GAZ</oboInOwl:hasOBONamespace>
        <oboInOwl:id>GAZ:00117964</oboInOwl:id>
        <rdfs:label>Usino Rural Local-Level Government Area</rdfs:label>
    </owl:NamedIndividual>
    


    <!-- http://purl.obolibrary.org/obo/GAZ_00117965 -->

    <owl:NamedIndividual rdf:about="http://purl.obolibrary.org/obo/GAZ_00117965">
        <obo:RO_0001025 rdf:resource="http://purl.obolibrary.org/obo/GAZ_00022350"/>
        <oboInOwl:hasOBONamespace>GAZ</oboInOwl:hasOBONamespace>
        <oboInOwl:id>GAZ:00117965</oboInOwl:id>
        <rdfs:label>Tunap-Hunstein Range Rural</rdfs:label>
    </owl:NamedIndividual>
    


    <!-- http://purl.obolibrary.org/obo/GAZ_00117966 -->

    <owl:NamedIndividual rdf:about="http://purl.obolibrary.org/obo/GAZ_00117966">
        <obo:RO_0001025 rdf:resource="http://purl.obolibrary.org/obo/GAZ_00022350"/>
        <oboInOwl:hasOBONamespace>GAZ</oboInOwl:hasOBONamespace>
        <oboInOwl:id>GAZ:00117966</oboInOwl:id>
        <rdfs:label>Ambunti Rural</rdfs:label>
    </owl:NamedIndividual>
    


    <!-- http://purl.obolibrary.org/obo/GAZ_00117967 -->

    <owl:NamedIndividual rdf:about="http://purl.obolibrary.org/obo/GAZ_00117967">
        <obo:RO_0001025 rdf:resource="http://purl.obolibrary.org/obo/GAZ_00022350"/>
        <oboInOwl:hasOBONamespace>GAZ</oboInOwl:hasOBONamespace>
        <oboInOwl:id>GAZ:00117967</oboInOwl:id>
        <rdfs:label>Dreikikir Rural</rdfs:label>
    </owl:NamedIndividual>
    


    <!-- http://purl.obolibrary.org/obo/GAZ_00117968 -->

    <owl:NamedIndividual rdf:about="http://purl.obolibrary.org/obo/GAZ_00117968">
        <obo:RO_0001025 rdf:resource="http://purl.obolibrary.org/obo/GAZ_00022350"/>
        <oboInOwl:hasOBONamespace>GAZ</oboInOwl:hasOBONamespace>
        <oboInOwl:id>GAZ:00117968</oboInOwl:id>
        <rdfs:label>Gawanga Rural</rdfs:label>
    </owl:NamedIndividual>
    


    <!-- http://purl.obolibrary.org/obo/GAZ_00117969 -->

    <owl:NamedIndividual rdf:about="http://purl.obolibrary.org/obo/GAZ_00117969">
        <obo:RO_0001025 rdf:resource="http://purl.obolibrary.org/obo/GAZ_00022349"/>
        <obo:IAO_0000115>A Local-Level Government Area of Angoram District.</obo:IAO_0000115>
        <oboInOwl:hasOBONamespace>GAZ</oboInOwl:hasOBONamespace>
        <oboInOwl:id>GAZ:00117969</oboInOwl:id>
        <rdfs:label>Angoram-Middle Sepik Rural Local-Level Government Area</rdfs:label>
    </owl:NamedIndividual>
    


    <!-- http://purl.obolibrary.org/obo/GAZ_00117970 -->

    <owl:NamedIndividual rdf:about="http://purl.obolibrary.org/obo/GAZ_00117970">
        <obo:RO_0001025 rdf:resource="http://purl.obolibrary.org/obo/GAZ_00022349"/>
        <obo:IAO_0000115>A Local-Level Government Area of Angoram District.</obo:IAO_0000115>
        <oboInOwl:hasOBONamespace>GAZ</oboInOwl:hasOBONamespace>
        <oboInOwl:id>GAZ:00117970</oboInOwl:id>
        <rdfs:label>Keram Rural Local-Level Government Area</rdfs:label>
    </owl:NamedIndividual>
    


    <!-- http://purl.obolibrary.org/obo/GAZ_00117971 -->

    <owl:NamedIndividual rdf:about="http://purl.obolibrary.org/obo/GAZ_00117971">
        <obo:RO_0001025 rdf:resource="http://purl.obolibrary.org/obo/GAZ_00022349"/>
        <obo:IAO_0000115>A Local-Level Government Area of Angoram District.</obo:IAO_0000115>
        <oboInOwl:hasOBONamespace>GAZ</oboInOwl:hasOBONamespace>
        <oboInOwl:id>GAZ:00117971</oboInOwl:id>
        <rdfs:label>Yuat Rural Local-Level Government Area</rdfs:label>
    </owl:NamedIndividual>
    


    <!-- http://purl.obolibrary.org/obo/GAZ_00117972 -->

    <owl:NamedIndividual rdf:about="http://purl.obolibrary.org/obo/GAZ_00117972">
        <obo:RO_0001025 rdf:resource="http://purl.obolibrary.org/obo/GAZ_00022349"/>
        <obo:IAO_0000115>A Local-Level Government Area of Angoram District.</obo:IAO_0000115>
        <oboInOwl:hasOBONamespace>GAZ</oboInOwl:hasOBONamespace>
        <oboInOwl:id>GAZ:00117972</oboInOwl:id>
        <rdfs:label>Marienberg-Lower Sepik Rural Local-Level Government Area</rdfs:label>
    </owl:NamedIndividual>
    


    <!-- http://purl.obolibrary.org/obo/GAZ_00117973 -->

    <owl:NamedIndividual rdf:about="http://purl.obolibrary.org/obo/GAZ_00117973">
        <obo:RO_0001025 rdf:resource="http://purl.obolibrary.org/obo/GAZ_00022349"/>
        <obo:IAO_0000115>A Local-Level Government Area of Angoram District.</obo:IAO_0000115>
        <oboInOwl:hasOBONamespace>GAZ</oboInOwl:hasOBONamespace>
        <oboInOwl:id>GAZ:00117973</oboInOwl:id>
        <rdfs:label>Karawari Rural Local-Level Government Area</rdfs:label>
    </owl:NamedIndividual>
    


    <!-- http://purl.obolibrary.org/obo/GAZ_00117974 -->

    <owl:NamedIndividual rdf:about="http://purl.obolibrary.org/obo/GAZ_00117974">
        <obo:RO_0001025 rdf:resource="http://purl.obolibrary.org/obo/GAZ_00022354"/>
        <obo:IAO_0000115>A Local-Level Government Area of Maprik District.</obo:IAO_0000115>
        <oboInOwl:hasOBONamespace>GAZ</oboInOwl:hasOBONamespace>
        <oboInOwl:id>GAZ:00117974</oboInOwl:id>
        <rdfs:label>Bumbuita Muhiang Rural Local-Level Government Area</rdfs:label>
    </owl:NamedIndividual>
    


    <!-- http://purl.obolibrary.org/obo/GAZ_00117975 -->

    <owl:NamedIndividual rdf:about="http://purl.obolibrary.org/obo/GAZ_00117975">
        <obo:RO_0001025 rdf:resource="http://purl.obolibrary.org/obo/GAZ_00022354"/>
        <obo:IAO_0000115>A Local-Level Government Area of Maprik District.</obo:IAO_0000115>
        <oboInOwl:hasOBONamespace>GAZ</oboInOwl:hasOBONamespace>
        <oboInOwl:id>GAZ:00117975</oboInOwl:id>
        <rdfs:label>Albiges Mamblep Rural Local-Level Government Area</rdfs:label>
    </owl:NamedIndividual>
    


    <!-- http://purl.obolibrary.org/obo/GAZ_00117976 -->

    <owl:NamedIndividual rdf:about="http://purl.obolibrary.org/obo/GAZ_00117976">
        <obo:RO_0001025 rdf:resource="http://purl.obolibrary.org/obo/GAZ_00022354"/>
        <obo:IAO_0000115>A Local-Level Government Area of Maprik District.</obo:IAO_0000115>
        <oboInOwl:hasOBONamespace>GAZ</oboInOwl:hasOBONamespace>
        <oboInOwl:id>GAZ:00117976</oboInOwl:id>
        <rdfs:label>Yamil Tamaui Rural Local-Level Government Area</rdfs:label>
    </owl:NamedIndividual>
    


    <!-- http://purl.obolibrary.org/obo/GAZ_00117977 -->

    <owl:NamedIndividual rdf:about="http://purl.obolibrary.org/obo/GAZ_00117977">
        <obo:RO_0001025 rdf:resource="http://purl.obolibrary.org/obo/GAZ_00022354"/>
        <obo:IAO_0000115>A Local-Level Government Area of Maprik District.</obo:IAO_0000115>
        <oboInOwl:hasOBONamespace>GAZ</oboInOwl:hasOBONamespace>
        <oboInOwl:id>GAZ:00117977</oboInOwl:id>
        <rdfs:label>Maprik Wora Rural Local-Level Government Area</rdfs:label>
    </owl:NamedIndividual>
    


    <!-- http://purl.obolibrary.org/obo/GAZ_00117978 -->

    <owl:NamedIndividual rdf:about="http://purl.obolibrary.org/obo/GAZ_00117978">
        <obo:RO_0001025 rdf:resource="http://purl.obolibrary.org/obo/GAZ_00022353"/>
        <obo:IAO_0000115>A Local-Level Government Area of Wosera-Gawi District.</obo:IAO_0000115>
        <oboInOwl:hasOBONamespace>GAZ</oboInOwl:hasOBONamespace>
        <oboInOwl:id>GAZ:00117978</oboInOwl:id>
        <rdfs:label>Burui-Kunai Rural Local-Level Government Area</rdfs:label>
    </owl:NamedIndividual>
    


    <!-- http://purl.obolibrary.org/obo/GAZ_00117979 -->

    <owl:NamedIndividual rdf:about="http://purl.obolibrary.org/obo/GAZ_00117979">
        <obo:RO_0001025 rdf:resource="http://purl.obolibrary.org/obo/GAZ_00022353"/>
        <obo:IAO_0000115>A Local-Level Government Area of Wosera-Gawi District.</obo:IAO_0000115>
        <oboInOwl:hasOBONamespace>GAZ</oboInOwl:hasOBONamespace>
        <oboInOwl:id>GAZ:00117979</oboInOwl:id>
        <rdfs:label>Gawi Rural Local-Level Government Area</rdfs:label>
    </owl:NamedIndividual>
    


    <!-- http://purl.obolibrary.org/obo/GAZ_00117980 -->

    <owl:NamedIndividual rdf:about="http://purl.obolibrary.org/obo/GAZ_00117980">
        <obo:RO_0001025 rdf:resource="http://purl.obolibrary.org/obo/GAZ_00022353"/>
        <obo:IAO_0000115>A Local-Level Government Area of Wosera-Gawi District.</obo:IAO_0000115>
        <oboInOwl:hasOBONamespace>GAZ</oboInOwl:hasOBONamespace>
        <oboInOwl:id>GAZ:00117980</oboInOwl:id>
        <rdfs:label>South Wosera Rural Local-Level Government Area</rdfs:label>
    </owl:NamedIndividual>
    


    <!-- http://purl.obolibrary.org/obo/GAZ_00117981 -->

    <owl:NamedIndividual rdf:about="http://purl.obolibrary.org/obo/GAZ_00117981">
        <obo:RO_0001025 rdf:resource="http://purl.obolibrary.org/obo/GAZ_00022353"/>
        <obo:IAO_0000115>A Local-Level Government Area of Wosera-Gawi District.</obo:IAO_0000115>
        <oboInOwl:hasOBONamespace>GAZ</oboInOwl:hasOBONamespace>
        <oboInOwl:id>GAZ:00117981</oboInOwl:id>
        <rdfs:label>North Wosera Rural Local-Level Government Area</rdfs:label>
    </owl:NamedIndividual>
    


    <!-- http://purl.obolibrary.org/obo/GAZ_00117982 -->

    <owl:NamedIndividual rdf:about="http://purl.obolibrary.org/obo/GAZ_00117982">
        <obo:RO_0001025 rdf:resource="http://purl.obolibrary.org/obo/GAZ_00022352"/>
        <obo:IAO_0000115>A Local-Level Government Area of Yangoru-Saussia District.</obo:IAO_0000115>
        <oboInOwl:hasOBONamespace>GAZ</oboInOwl:hasOBONamespace>
        <oboInOwl:id>GAZ:00117982</oboInOwl:id>
        <rdfs:label>Numbo Rural Local-Level Government Area</rdfs:label>
    </owl:NamedIndividual>
    


    <!-- http://purl.obolibrary.org/obo/GAZ_00117983 -->

    <owl:NamedIndividual rdf:about="http://purl.obolibrary.org/obo/GAZ_00117983">
        <obo:RO_0001025 rdf:resource="http://purl.obolibrary.org/obo/GAZ_00022352"/>
        <obo:IAO_0000115>A Local-Level Government Area of Yangoru-Saussia District.</obo:IAO_0000115>
        <oboInOwl:hasOBONamespace>GAZ</oboInOwl:hasOBONamespace>
        <oboInOwl:id>GAZ:00117983</oboInOwl:id>
        <rdfs:label>Sausso Rural Local-Level Government Area</rdfs:label>
    </owl:NamedIndividual>
    


    <!-- http://purl.obolibrary.org/obo/GAZ_00117984 -->

    <owl:NamedIndividual rdf:about="http://purl.obolibrary.org/obo/GAZ_00117984">
        <obo:RO_0001025 rdf:resource="http://purl.obolibrary.org/obo/GAZ_00022352"/>
        <obo:IAO_0000115>A Local-Level Government Area of Yangoru-Saussia District.</obo:IAO_0000115>
        <oboInOwl:hasOBONamespace>GAZ</oboInOwl:hasOBONamespace>
        <oboInOwl:id>GAZ:00117984</oboInOwl:id>
        <rdfs:label>West Yangoru Rural Local-Level Government Area</rdfs:label>
    </owl:NamedIndividual>
    


    <!-- http://purl.obolibrary.org/obo/GAZ_00117985 -->

    <owl:NamedIndividual rdf:about="http://purl.obolibrary.org/obo/GAZ_00117985">
        <obo:RO_0001025 rdf:resource="http://purl.obolibrary.org/obo/GAZ_00022352"/>
        <obo:IAO_0000115>A Local-Level Government Area of Yangoru-Saussia District.</obo:IAO_0000115>
        <oboInOwl:hasOBONamespace>GAZ</oboInOwl:hasOBONamespace>
        <oboInOwl:id>GAZ:00117985</oboInOwl:id>
        <rdfs:label>East Yangoru Rural Local-Level Government Area</rdfs:label>
    </owl:NamedIndividual>
    


    <!-- http://purl.obolibrary.org/obo/GAZ_00117986 -->

    <owl:NamedIndividual rdf:about="http://purl.obolibrary.org/obo/GAZ_00117986">
        <obo:RO_0001025 rdf:resource="http://purl.obolibrary.org/obo/GAZ_00022430"/>
        <obo:IAO_0000115>A Local-Level Government Area of Aitape-Lumi District.</obo:IAO_0000115>
        <oboInOwl:hasOBONamespace>GAZ</oboInOwl:hasOBONamespace>
        <oboInOwl:id>GAZ:00117986</oboInOwl:id>
        <rdfs:label>West Aitape Rural Local-Level Government Area</rdfs:label>
    </owl:NamedIndividual>
    


    <!-- http://purl.obolibrary.org/obo/GAZ_00117987 -->

    <owl:NamedIndividual rdf:about="http://purl.obolibrary.org/obo/GAZ_00117987">
        <obo:RO_0001025 rdf:resource="http://purl.obolibrary.org/obo/GAZ_00022430"/>
        <obo:IAO_0000115>A Local-Level Government Area of Aitape-Lumi District.</obo:IAO_0000115>
        <oboInOwl:hasOBONamespace>GAZ</oboInOwl:hasOBONamespace>
        <oboInOwl:id>GAZ:00117987</oboInOwl:id>
        <rdfs:label>West Wapei Rural Local-Level Government Area</rdfs:label>
    </owl:NamedIndividual>
    


    <!-- http://purl.obolibrary.org/obo/GAZ_00117988 -->

    <owl:NamedIndividual rdf:about="http://purl.obolibrary.org/obo/GAZ_00117988">
        <obo:RO_0001025 rdf:resource="http://purl.obolibrary.org/obo/GAZ_00022430"/>
        <obo:IAO_0000115>A Local-Level Government Area of Aitape-Lumi District.</obo:IAO_0000115>
        <oboInOwl:hasOBONamespace>GAZ</oboInOwl:hasOBONamespace>
        <oboInOwl:id>GAZ:00117988</oboInOwl:id>
        <rdfs:label>East Aitape Rural Local-Level Government Area</rdfs:label>
    </owl:NamedIndividual>
    


    <!-- http://purl.obolibrary.org/obo/GAZ_00117989 -->

    <owl:NamedIndividual rdf:about="http://purl.obolibrary.org/obo/GAZ_00117989">
        <obo:RO_0001025 rdf:resource="http://purl.obolibrary.org/obo/GAZ_00022430"/>
        <obo:IAO_0000115>A Local-Level Government Area of Aitape-Lumi District.</obo:IAO_0000115>
        <oboInOwl:hasOBONamespace>GAZ</oboInOwl:hasOBONamespace>
        <oboInOwl:id>GAZ:00117989</oboInOwl:id>
        <rdfs:label>East Wapei Rural Local-Level Government Area</rdfs:label>
    </owl:NamedIndividual>
    


    <!-- http://purl.obolibrary.org/obo/GAZ_00117990 -->

    <owl:NamedIndividual rdf:about="http://purl.obolibrary.org/obo/GAZ_00117990">
        <obo:RO_0001025 rdf:resource="http://purl.obolibrary.org/obo/GAZ_00022431"/>
        <obo:IAO_0000115>A Local-Level Government Area of Nuku District.</obo:IAO_0000115>
        <oboInOwl:hasOBONamespace>GAZ</oboInOwl:hasOBONamespace>
        <oboInOwl:id>GAZ:00117990</oboInOwl:id>
        <rdfs:label>Nuku Rural Local-Level Government Area</rdfs:label>
    </owl:NamedIndividual>
    


    <!-- http://purl.obolibrary.org/obo/GAZ_00117991 -->

    <owl:NamedIndividual rdf:about="http://purl.obolibrary.org/obo/GAZ_00117991">
        <obo:RO_0001025 rdf:resource="http://purl.obolibrary.org/obo/GAZ_00022431"/>
        <obo:IAO_0000115>A Local-Level Government Area of Nuku District.</obo:IAO_0000115>
        <oboInOwl:hasOBONamespace>GAZ</oboInOwl:hasOBONamespace>
        <oboInOwl:id>GAZ:00117991</oboInOwl:id>
        <rdfs:label>Yangkok Rural Local-Level Government Area</rdfs:label>
    </owl:NamedIndividual>
    


    <!-- http://purl.obolibrary.org/obo/GAZ_00117992 -->

    <owl:NamedIndividual rdf:about="http://purl.obolibrary.org/obo/GAZ_00117992">
        <obo:RO_0001025 rdf:resource="http://purl.obolibrary.org/obo/GAZ_00022431"/>
        <obo:IAO_0000115>A Local-Level Government Area of Nuku District.</obo:IAO_0000115>
        <oboInOwl:hasOBONamespace>GAZ</oboInOwl:hasOBONamespace>
        <oboInOwl:id>GAZ:00117992</oboInOwl:id>
        <rdfs:label>Palai Rural Local-Level Government Area</rdfs:label>
    </owl:NamedIndividual>
    


    <!-- http://purl.obolibrary.org/obo/GAZ_00117993 -->

    <owl:NamedIndividual rdf:about="http://purl.obolibrary.org/obo/GAZ_00117993">
        <obo:RO_0001025 rdf:resource="http://purl.obolibrary.org/obo/GAZ_00022431"/>
        <obo:IAO_0000115>A Local-Level Government Area of Nuku District.</obo:IAO_0000115>
        <oboInOwl:hasOBONamespace>GAZ</oboInOwl:hasOBONamespace>
        <oboInOwl:id>GAZ:00117993</oboInOwl:id>
        <rdfs:label>Maimai Wanwan Rural Local-Level Government Area</rdfs:label>
    </owl:NamedIndividual>
    


    <!-- http://purl.obolibrary.org/obo/GAZ_00117994 -->

    <owl:NamedIndividual rdf:about="http://purl.obolibrary.org/obo/GAZ_00117994">
        <obo:RO_0001025 rdf:resource="http://purl.obolibrary.org/obo/GAZ_00022433"/>
        <obo:IAO_0000115>A Local-Level Government Area of Telefomin District.</obo:IAO_0000115>
        <oboInOwl:hasOBONamespace>GAZ</oboInOwl:hasOBONamespace>
        <oboInOwl:id>GAZ:00117994</oboInOwl:id>
        <rdfs:label>Namea Rural Local-Level Government Area</rdfs:label>
    </owl:NamedIndividual>
    


    <!-- http://purl.obolibrary.org/obo/GAZ_00117995 -->

    <owl:NamedIndividual rdf:about="http://purl.obolibrary.org/obo/GAZ_00117995">
        <obo:RO_0001025 rdf:resource="http://purl.obolibrary.org/obo/GAZ_00022433"/>
        <obo:IAO_0000115>A Local-Level Government Area of Telefomin District.</obo:IAO_0000115>
        <oboInOwl:hasOBONamespace>GAZ</oboInOwl:hasOBONamespace>
        <oboInOwl:id>GAZ:00117995</oboInOwl:id>
        <rdfs:label>Oksapmin Rural Local-Level Government Area</rdfs:label>
    </owl:NamedIndividual>
    


    <!-- http://purl.obolibrary.org/obo/GAZ_00117996 -->

    <owl:NamedIndividual rdf:about="http://purl.obolibrary.org/obo/GAZ_00117996">
        <obo:RO_0001025 rdf:resource="http://purl.obolibrary.org/obo/GAZ_00022433"/>
        <obo:IAO_0000115>A Local-Level Government Area of Telefomin District.</obo:IAO_0000115>
        <oboInOwl:hasOBONamespace>GAZ</oboInOwl:hasOBONamespace>
        <oboInOwl:id>GAZ:00117996</oboInOwl:id>
        <rdfs:label>Telefomin Rural Local-Level Government Area</rdfs:label>
    </owl:NamedIndividual>
    


    <!-- http://purl.obolibrary.org/obo/GAZ_00117997 -->

    <owl:NamedIndividual rdf:about="http://purl.obolibrary.org/obo/GAZ_00117997">
        <obo:RO_0001025 rdf:resource="http://purl.obolibrary.org/obo/GAZ_00022433"/>
        <obo:IAO_0000115>A Local-Level Government Area of Telefomin District.</obo:IAO_0000115>
        <oboInOwl:hasOBONamespace>GAZ</oboInOwl:hasOBONamespace>
        <oboInOwl:id>GAZ:00117997</oboInOwl:id>
        <rdfs:label>Yapsie Rural Local-Level Government Area</rdfs:label>
    </owl:NamedIndividual>
    


    <!-- http://purl.obolibrary.org/obo/GAZ_00117998 -->

    <owl:NamedIndividual rdf:about="http://purl.obolibrary.org/obo/GAZ_00117998">
        <obo:RO_0001025 rdf:resource="http://purl.obolibrary.org/obo/GAZ_00022432"/>
        <obo:IAO_0000115>A Local-Level Government Area of Vanimo-Green River District.</obo:IAO_0000115>
        <oboInOwl:hasOBONamespace>GAZ</oboInOwl:hasOBONamespace>
        <oboInOwl:id>GAZ:00117998</oboInOwl:id>
        <rdfs:label>Amanab Rural Local-Level Government Area</rdfs:label>
    </owl:NamedIndividual>
    


    <!-- http://purl.obolibrary.org/obo/GAZ_00117999 -->

    <owl:NamedIndividual rdf:about="http://purl.obolibrary.org/obo/GAZ_00117999">
        <obo:RO_0001025 rdf:resource="http://purl.obolibrary.org/obo/GAZ_00022432"/>
        <obo:IAO_0000115>A Local-Level Government Area of Vanimo-Green River District.</obo:IAO_0000115>
        <oboInOwl:hasOBONamespace>GAZ</oboInOwl:hasOBONamespace>
        <oboInOwl:id>GAZ:00117999</oboInOwl:id>
        <rdfs:label>Green River Rural Local-Level Government Area</rdfs:label>
    </owl:NamedIndividual>
    


    <!-- http://purl.obolibrary.org/obo/GAZ_00118000 -->

    <owl:NamedIndividual rdf:about="http://purl.obolibrary.org/obo/GAZ_00118000">
        <obo:RO_0001025 rdf:resource="http://purl.obolibrary.org/obo/GAZ_00022432"/>
        <obo:IAO_0000115>A Local-Level Government Area of Vanimo-Green River District.</obo:IAO_0000115>
        <oboInOwl:hasOBONamespace>GAZ</oboInOwl:hasOBONamespace>
        <oboInOwl:id>GAZ:00118000</oboInOwl:id>
        <rdfs:label>Walsa Rural Local-Level Government Area</rdfs:label>
    </owl:NamedIndividual>
    


    <!-- http://purl.obolibrary.org/obo/GAZ_00118001 -->

    <owl:NamedIndividual rdf:about="http://purl.obolibrary.org/obo/GAZ_00118001">
        <obo:RO_0001025 rdf:resource="http://purl.obolibrary.org/obo/GAZ_00022432"/>
        <obo:IAO_0000115>A Local-Level Government Area of Vanimo-Green River District.</obo:IAO_0000115>
        <oboInOwl:hasOBONamespace>GAZ</oboInOwl:hasOBONamespace>
        <oboInOwl:id>GAZ:00118001</oboInOwl:id>
        <rdfs:label>Vanimo Urban Local-Level Government Area</rdfs:label>
    </owl:NamedIndividual>
    


    <!-- http://purl.obolibrary.org/obo/GAZ_00118002 -->

    <owl:NamedIndividual rdf:about="http://purl.obolibrary.org/obo/GAZ_00118002">
        <obo:RO_0001025 rdf:resource="http://purl.obolibrary.org/obo/GAZ_00022432"/>
        <obo:IAO_0000115>A Local-Level Government Area of Vanimo-Green River District.</obo:IAO_0000115>
        <oboInOwl:hasOBONamespace>GAZ</oboInOwl:hasOBONamespace>
        <oboInOwl:id>GAZ:00118002</oboInOwl:id>
        <rdfs:label>Bewani-Wutung-Onei Rural Local-Level Government Area</rdfs:label>
    </owl:NamedIndividual>
    


    <!-- http://purl.obolibrary.org/obo/GAZ_00118003 -->

    <owl:NamedIndividual rdf:about="http://purl.obolibrary.org/obo/GAZ_00118003">
        <obo:RO_0001025 rdf:resource="http://purl.obolibrary.org/obo/GAZ_00022335"/>
        <obo:IAO_0000115>A Local-Level Government Area of Abau District.</obo:IAO_0000115>
        <oboInOwl:hasOBONamespace>GAZ</oboInOwl:hasOBONamespace>
        <oboInOwl:id>GAZ:00118003</oboInOwl:id>
        <rdfs:label>Amazon Bay Rural Local-Level Government Area</rdfs:label>
    </owl:NamedIndividual>
    


    <!-- http://purl.obolibrary.org/obo/GAZ_00118004 -->

    <owl:NamedIndividual rdf:about="http://purl.obolibrary.org/obo/GAZ_00118004">
        <obo:RO_0001025 rdf:resource="http://purl.obolibrary.org/obo/GAZ_00022355"/>
        <obo:IAO_0000115>A Local-Level Government Area of Kerema District.</obo:IAO_0000115>
        <oboInOwl:hasOBONamespace>GAZ</oboInOwl:hasOBONamespace>
        <oboInOwl:id>GAZ:00118004</oboInOwl:id>
        <rdfs:label>Kaintiba Rural Local-Level Government Area</rdfs:label>
    </owl:NamedIndividual>
    


    <!-- http://purl.obolibrary.org/obo/GAZ_00118005 -->

    <owl:NamedIndividual rdf:about="http://purl.obolibrary.org/obo/GAZ_00118005">
        <obo:RO_0001025 rdf:resource="http://purl.obolibrary.org/obo/GAZ_00022335"/>
        <obo:IAO_0000115>A Local-Level Government Area of Abau District.</obo:IAO_0000115>
        <oboInOwl:hasOBONamespace>GAZ</oboInOwl:hasOBONamespace>
        <oboInOwl:id>GAZ:00118005</oboInOwl:id>
        <rdfs:label>Aroma Rural Local-Level Government Area</rdfs:label>
    </owl:NamedIndividual>
    


    <!-- http://purl.obolibrary.org/obo/GAZ_00118006 -->

    <owl:NamedIndividual rdf:about="http://purl.obolibrary.org/obo/GAZ_00118006">
        <obo:RO_0001025 rdf:resource="http://purl.obolibrary.org/obo/GAZ_00022335"/>
        <obo:IAO_0000115>A Local-Level Government Area of Abau District.</obo:IAO_0000115>
        <oboInOwl:hasOBONamespace>GAZ</oboInOwl:hasOBONamespace>
        <oboInOwl:id>GAZ:00118006</oboInOwl:id>
        <rdfs:label>Cloudy Bay Rural Local-Level Government Area</rdfs:label>
    </owl:NamedIndividual>
    


    <!-- http://purl.obolibrary.org/obo/GAZ_00118007 -->

    <owl:NamedIndividual rdf:about="http://purl.obolibrary.org/obo/GAZ_00118007">
        <obo:RO_0001025 rdf:resource="http://purl.obolibrary.org/obo/GAZ_00022336"/>
        <obo:IAO_0000115>A Local-Level Government Area of Goilala District.</obo:IAO_0000115>
        <oboInOwl:hasOBONamespace>GAZ</oboInOwl:hasOBONamespace>
        <oboInOwl:id>GAZ:00118007</oboInOwl:id>
        <rdfs:label>Woitape Rural Local-Level Government Area</rdfs:label>
    </owl:NamedIndividual>
    


    <!-- http://purl.obolibrary.org/obo/GAZ_00118008 -->

    <owl:NamedIndividual rdf:about="http://purl.obolibrary.org/obo/GAZ_00118008">
        <obo:RO_0001025 rdf:resource="http://purl.obolibrary.org/obo/GAZ_00022336"/>
        <obo:IAO_0000115>A Local-Level Government Area of Goilala District.</obo:IAO_0000115>
        <oboInOwl:hasOBONamespace>GAZ</oboInOwl:hasOBONamespace>
        <oboInOwl:id>GAZ:00118008</oboInOwl:id>
        <rdfs:label>Tapini Rural Local-Level Government Area</rdfs:label>
    </owl:NamedIndividual>
    


    <!-- http://purl.obolibrary.org/obo/GAZ_00118009 -->

    <owl:NamedIndividual rdf:about="http://purl.obolibrary.org/obo/GAZ_00118009">
        <obo:RO_0001025 rdf:resource="http://purl.obolibrary.org/obo/GAZ_00022336"/>
        <obo:IAO_0000115>A Local-Level Government Area of Goilala District.</obo:IAO_0000115>
        <oboInOwl:hasOBONamespace>GAZ</oboInOwl:hasOBONamespace>
        <oboInOwl:id>GAZ:00118009</oboInOwl:id>
        <rdfs:label>Guari Rural Local-Level Government Area</rdfs:label>
    </owl:NamedIndividual>
    


    <!-- http://purl.obolibrary.org/obo/GAZ_00118010 -->

    <owl:NamedIndividual rdf:about="http://purl.obolibrary.org/obo/GAZ_00118010">
        <obo:RO_0001025 rdf:resource="http://purl.obolibrary.org/obo/GAZ_00022333"/>
        <obo:IAO_0000115>A Local-Level Government Area of Kairuku-Hiri District.</obo:IAO_0000115>
        <oboInOwl:hasOBONamespace>GAZ</oboInOwl:hasOBONamespace>
        <oboInOwl:id>GAZ:00118010</oboInOwl:id>
        <rdfs:label>Kairuku Rural Local-Level Government Area</rdfs:label>
    </owl:NamedIndividual>
    


    <!-- http://purl.obolibrary.org/obo/GAZ_00118011 -->

    <owl:NamedIndividual rdf:about="http://purl.obolibrary.org/obo/GAZ_00118011">
        <obo:RO_0001025 rdf:resource="http://purl.obolibrary.org/obo/GAZ_00022333"/>
        <obo:IAO_0000115>A Local-Level Government Area of Kairuku-Hiri District.</obo:IAO_0000115>
        <oboInOwl:hasOBONamespace>GAZ</oboInOwl:hasOBONamespace>
        <oboInOwl:id>GAZ:00118011</oboInOwl:id>
        <rdfs:label>Mekeo Kuni Rural Local-Level Government Area</rdfs:label>
    </owl:NamedIndividual>
    


    <!-- http://purl.obolibrary.org/obo/GAZ_00118012 -->

    <owl:NamedIndividual rdf:about="http://purl.obolibrary.org/obo/GAZ_00118012">
        <obo:RO_0001025 rdf:resource="http://purl.obolibrary.org/obo/GAZ_00022333"/>
        <obo:IAO_0000115>A Local-Level Government Area of Kairuku-Hiri District.</obo:IAO_0000115>
        <oboInOwl:hasOBONamespace>GAZ</oboInOwl:hasOBONamespace>
        <oboInOwl:id>GAZ:00118012</oboInOwl:id>
        <rdfs:label>Hiri Rural Local-Level Government Area</rdfs:label>
    </owl:NamedIndividual>
    


    <!-- http://purl.obolibrary.org/obo/GAZ_00118013 -->

    <owl:NamedIndividual rdf:about="http://purl.obolibrary.org/obo/GAZ_00118013">
        <obo:RO_0001025 rdf:resource="http://purl.obolibrary.org/obo/GAZ_00022333"/>
        <obo:IAO_0000115>A Local-Level Government Area of Kairuku-Hiri District.</obo:IAO_0000115>
        <oboInOwl:hasOBONamespace>GAZ</oboInOwl:hasOBONamespace>
        <oboInOwl:id>GAZ:00118013</oboInOwl:id>
        <rdfs:label>Koiari Rural Local-Level Government Area</rdfs:label>
    </owl:NamedIndividual>
    


    <!-- http://purl.obolibrary.org/obo/GAZ_00118014 -->

    <owl:NamedIndividual rdf:about="http://purl.obolibrary.org/obo/GAZ_00118014">
        <obo:RO_0001025 rdf:resource="http://purl.obolibrary.org/obo/GAZ_00022334"/>
        <obo:IAO_0000115>A Local-Level Government Area of Rigo District.</obo:IAO_0000115>
        <oboInOwl:hasOBONamespace>GAZ</oboInOwl:hasOBONamespace>
        <oboInOwl:id>GAZ:00118014</oboInOwl:id>
        <rdfs:label>Rigo Central Rural Local-Level Government Area</rdfs:label>
    </owl:NamedIndividual>
    


    <!-- http://purl.obolibrary.org/obo/GAZ_00118015 -->

    <owl:NamedIndividual rdf:about="http://purl.obolibrary.org/obo/GAZ_00118015">
        <obo:RO_0001025 rdf:resource="http://purl.obolibrary.org/obo/GAZ_00022334"/>
        <obo:IAO_0000115>A Local-Level Government Area of Rigo District.</obo:IAO_0000115>
        <oboInOwl:hasOBONamespace>GAZ</oboInOwl:hasOBONamespace>
        <oboInOwl:id>GAZ:00118015</oboInOwl:id>
        <rdfs:label>Rigo Inland Rural Local-Level Government Area</rdfs:label>
    </owl:NamedIndividual>
    


    <!-- http://purl.obolibrary.org/obo/GAZ_00118016 -->

    <owl:NamedIndividual rdf:about="http://purl.obolibrary.org/obo/GAZ_00118016">
        <obo:RO_0001025 rdf:resource="http://purl.obolibrary.org/obo/GAZ_00022334"/>
        <obo:IAO_0000115>A Local-Level Government Area of Rigo District.</obo:IAO_0000115>
        <oboInOwl:hasOBONamespace>GAZ</oboInOwl:hasOBONamespace>
        <oboInOwl:id>GAZ:00118016</oboInOwl:id>
        <rdfs:label>Rigo Coastal Rural Local-Level Government Area</rdfs:label>
    </owl:NamedIndividual>
    


    <!-- http://purl.obolibrary.org/obo/GAZ_00118017 -->

    <owl:NamedIndividual rdf:about="http://purl.obolibrary.org/obo/GAZ_00118017">
        <obo:RO_0001025 rdf:resource="http://purl.obolibrary.org/obo/GAZ_00022355"/>
        <obo:IAO_0000115>A Local-Level Government Area of Kerema District.</obo:IAO_0000115>
        <oboInOwl:hasOBONamespace>GAZ</oboInOwl:hasOBONamespace>
        <oboInOwl:id>GAZ:00118017</oboInOwl:id>
        <rdfs:label>East Kerema Rural Local-Level Government Area</rdfs:label>
    </owl:NamedIndividual>
    


    <!-- http://purl.obolibrary.org/obo/GAZ_00118018 -->

    <owl:NamedIndividual rdf:about="http://purl.obolibrary.org/obo/GAZ_00118018">
        <obo:RO_0001025 rdf:resource="http://purl.obolibrary.org/obo/GAZ_00022355"/>
        <obo:IAO_0000115>A Local-Level Government Area of Kerema District.</obo:IAO_0000115>
        <oboInOwl:hasOBONamespace>GAZ</oboInOwl:hasOBONamespace>
        <oboInOwl:id>GAZ:00118018</oboInOwl:id>
        <rdfs:label>Lakekamu-Tauri Rural Local-Level Government Area</rdfs:label>
    </owl:NamedIndividual>
    


    <!-- http://purl.obolibrary.org/obo/GAZ_00118019 -->

    <owl:NamedIndividual rdf:about="http://purl.obolibrary.org/obo/GAZ_00118019">
        <obo:RO_0001025 rdf:resource="http://purl.obolibrary.org/obo/GAZ_00022355"/>
        <obo:IAO_0000115>A Local-Level Government Area of Kerema District.</obo:IAO_0000115>
        <oboInOwl:hasOBONamespace>GAZ</oboInOwl:hasOBONamespace>
        <oboInOwl:id>GAZ:00118019</oboInOwl:id>
        <rdfs:label>Central Kerema Rural Local-Level Government Area</rdfs:label>
    </owl:NamedIndividual>
    


    <!-- http://purl.obolibrary.org/obo/GAZ_00118020 -->

    <owl:NamedIndividual rdf:about="http://purl.obolibrary.org/obo/GAZ_00118020">
        <obo:RO_0001025 rdf:resource="http://purl.obolibrary.org/obo/GAZ_00022355"/>
        <obo:IAO_0000115>A Local-Level Government Area of Kerema District.</obo:IAO_0000115>
        <oboInOwl:hasOBONamespace>GAZ</oboInOwl:hasOBONamespace>
        <oboInOwl:id>GAZ:00118020</oboInOwl:id>
        <rdfs:label>Kotidanga Rural Local-Level Government Area</rdfs:label>
    </owl:NamedIndividual>
    


    <!-- http://purl.obolibrary.org/obo/GAZ_00118021 -->

    <owl:NamedIndividual rdf:about="http://purl.obolibrary.org/obo/GAZ_00118021">
        <obo:RO_0001025 rdf:resource="http://purl.obolibrary.org/obo/GAZ_00022355"/>
        <obo:IAO_0000115>A Local-Level Government Area of Kerema District.</obo:IAO_0000115>
        <oboInOwl:hasOBONamespace>GAZ</oboInOwl:hasOBONamespace>
        <oboInOwl:id>GAZ:00118021</oboInOwl:id>
        <rdfs:label>Kerema Urban Local-Level Government Area</rdfs:label>
    </owl:NamedIndividual>
    


    <!-- http://purl.obolibrary.org/obo/GAZ_00118022 -->

    <owl:NamedIndividual rdf:about="http://purl.obolibrary.org/obo/GAZ_00118022">
        <obo:RO_0001025 rdf:resource="http://purl.obolibrary.org/obo/GAZ_00022360"/>
        <obo:IAO_0000115>A Local-Level Government Area of Kikori District.</obo:IAO_0000115>
        <oboInOwl:hasOBONamespace>GAZ</oboInOwl:hasOBONamespace>
        <oboInOwl:id>GAZ:00118022</oboInOwl:id>
        <rdfs:label>Baimuru Rural Local-Level Government Area</rdfs:label>
    </owl:NamedIndividual>
    


    <!-- http://purl.obolibrary.org/obo/GAZ_00118023 -->

    <owl:NamedIndividual rdf:about="http://purl.obolibrary.org/obo/GAZ_00118023">
        <obo:RO_0001025 rdf:resource="http://purl.obolibrary.org/obo/GAZ_00022360"/>
        <obo:IAO_0000115>A Local-Level Government Area of Kikori District.</obo:IAO_0000115>
        <oboInOwl:hasOBONamespace>GAZ</oboInOwl:hasOBONamespace>
        <oboInOwl:id>GAZ:00118023</oboInOwl:id>
        <rdfs:label>West Kikori Rural Local-Level Government Area</rdfs:label>
    </owl:NamedIndividual>
    


    <!-- http://purl.obolibrary.org/obo/GAZ_00118024 -->

    <owl:NamedIndividual rdf:about="http://purl.obolibrary.org/obo/GAZ_00118024">
        <obo:RO_0001025 rdf:resource="http://purl.obolibrary.org/obo/GAZ_00022360"/>
        <obo:IAO_0000115>A Local-Level Government Area of Kikori District.</obo:IAO_0000115>
        <oboInOwl:hasOBONamespace>GAZ</oboInOwl:hasOBONamespace>
        <oboInOwl:id>GAZ:00118024</oboInOwl:id>
        <rdfs:label>Ihu Rural Local-Level Government Area</rdfs:label>
    </owl:NamedIndividual>
    


    <!-- http://purl.obolibrary.org/obo/GAZ_00118025 -->

    <owl:NamedIndividual rdf:about="http://purl.obolibrary.org/obo/GAZ_00118025">
        <obo:RO_0001025 rdf:resource="http://purl.obolibrary.org/obo/GAZ_00022360"/>
        <obo:IAO_0000115>A Local-Level Government Area of Kikori District.</obo:IAO_0000115>
        <oboInOwl:hasOBONamespace>GAZ</oboInOwl:hasOBONamespace>
        <oboInOwl:id>GAZ:00118025</oboInOwl:id>
        <rdfs:label>East Kikori Rural Local-Level Government Area</rdfs:label>
    </owl:NamedIndividual>
    


    <!-- http://purl.obolibrary.org/obo/GAZ_00118026 -->

    <owl:NamedIndividual rdf:about="http://purl.obolibrary.org/obo/GAZ_00118026">
        <obo:RO_0001025 rdf:resource="http://purl.obolibrary.org/obo/GAZ_00022379"/>
        <obo:RO_0001025 rdf:resource="http://purl.obolibrary.org/obo/GAZ_00051599"/>
        <obo:IAO_0000115>An island in Samarai-Murua District.</obo:IAO_0000115>
        <oboInOwl:hasOBONamespace>GAZ</oboInOwl:hasOBONamespace>
        <oboInOwl:id>GAZ:00118026</oboInOwl:id>
        <rdfs:label>Calvados Island</rdfs:label>
    </owl:NamedIndividual>
    


    <!-- http://purl.obolibrary.org/obo/GAZ_00118027 -->

    <owl:NamedIndividual rdf:about="http://purl.obolibrary.org/obo/GAZ_00118027">
        <obo:RO_0001025 rdf:resource="http://purl.obolibrary.org/obo/GAZ_00051597"/>
        <obo:IAO_0000115>One of the Engineer Islands.</obo:IAO_0000115>
        <oboInOwl:hasOBONamespace>GAZ</oboInOwl:hasOBONamespace>
        <oboInOwl:id>GAZ:00118027</oboInOwl:id>
        <rdfs:label>Tubetube Island</rdfs:label>
    </owl:NamedIndividual>
    


    <!-- http://purl.obolibrary.org/obo/GAZ_00118028 -->

    <owl:NamedIndividual rdf:about="http://purl.obolibrary.org/obo/GAZ_00118028">
        <obo:RO_0001025 rdf:resource="http://purl.obolibrary.org/obo/GAZ_00051597"/>
        <obo:IAO_0000115>One of the Engineer Islands.</obo:IAO_0000115>
        <oboInOwl:hasOBONamespace>GAZ</oboInOwl:hasOBONamespace>
        <oboInOwl:id>GAZ:00118028</oboInOwl:id>
        <rdfs:label>Koraiwe Island</rdfs:label>
    </owl:NamedIndividual>
    


    <!-- http://purl.obolibrary.org/obo/GAZ_00118029 -->

    <owl:NamedIndividual rdf:about="http://purl.obolibrary.org/obo/GAZ_00118029">
        <obo:RO_0001025 rdf:resource="http://purl.obolibrary.org/obo/GAZ_00007183"/>
        <obo:IAO_0000115>The largest of the Trobriand Islands. It is part of the Milne Bay Province of Papua New Guinea.</obo:IAO_0000115>
        <oboInOwl:hasOBONamespace>GAZ</oboInOwl:hasOBONamespace>
        <oboInOwl:id>GAZ:00118029</oboInOwl:id>
        <rdfs:label>Kiriwina Island</rdfs:label>
    </owl:NamedIndividual>
    


    <!-- http://purl.obolibrary.org/obo/GAZ_00118030 -->

    <owl:NamedIndividual rdf:about="http://purl.obolibrary.org/obo/GAZ_00118030">
        <obo:RO_0001025 rdf:resource="http://purl.obolibrary.org/obo/GAZ_00022381"/>
        <obo:IAO_0000115>A Local-Level Government Area of Alotau District.</obo:IAO_0000115>
        <oboInOwl:hasOBONamespace>GAZ</oboInOwl:hasOBONamespace>
        <oboInOwl:id>GAZ:00118030</oboInOwl:id>
        <rdfs:label>Makamaka Rural Local-Level Government Area</rdfs:label>
    </owl:NamedIndividual>
    


    <!-- http://purl.obolibrary.org/obo/GAZ_00118031 -->

    <owl:NamedIndividual rdf:about="http://purl.obolibrary.org/obo/GAZ_00118031">
        <obo:RO_0001025 rdf:resource="http://purl.obolibrary.org/obo/GAZ_00022381"/>
        <obo:IAO_0000115>A Local-Level Government Area of Alotau District.</obo:IAO_0000115>
        <oboInOwl:hasOBONamespace>GAZ</oboInOwl:hasOBONamespace>
        <oboInOwl:id>GAZ:00118031</oboInOwl:id>
        <rdfs:label>Daga Rural Local-Level Government Area</rdfs:label>
    </owl:NamedIndividual>
    


    <!-- http://purl.obolibrary.org/obo/GAZ_00118032 -->

    <owl:NamedIndividual rdf:about="http://purl.obolibrary.org/obo/GAZ_00118032">
        <obo:RO_0001025 rdf:resource="http://purl.obolibrary.org/obo/GAZ_00022381"/>
        <obo:IAO_0000115>A Local-Level Government Area of Alotau District.</obo:IAO_0000115>
        <oboInOwl:hasOBONamespace>GAZ</oboInOwl:hasOBONamespace>
        <oboInOwl:id>GAZ:00118032</oboInOwl:id>
        <rdfs:label>Weraura Rural Local-Level Government Area</rdfs:label>
    </owl:NamedIndividual>
    


    <!-- http://purl.obolibrary.org/obo/GAZ_00118033 -->

    <owl:NamedIndividual rdf:about="http://purl.obolibrary.org/obo/GAZ_00118033">
        <obo:RO_0001025 rdf:resource="http://purl.obolibrary.org/obo/GAZ_00022381"/>
        <obo:IAO_0000115>A Local-Level Government Area of Alotau District.</obo:IAO_0000115>
        <oboInOwl:hasOBONamespace>GAZ</oboInOwl:hasOBONamespace>
        <oboInOwl:id>GAZ:00118033</oboInOwl:id>
        <rdfs:label>Maramatana Rural Local-Level Government Area</rdfs:label>
    </owl:NamedIndividual>
    


    <!-- http://purl.obolibrary.org/obo/GAZ_00118034 -->

    <owl:NamedIndividual rdf:about="http://purl.obolibrary.org/obo/GAZ_00118034">
        <obo:RO_0001025 rdf:resource="http://purl.obolibrary.org/obo/GAZ_00022381"/>
        <obo:IAO_0000115>A Local-Level Government Area of Alotau District.</obo:IAO_0000115>
        <oboInOwl:hasOBONamespace>GAZ</oboInOwl:hasOBONamespace>
        <oboInOwl:id>GAZ:00118034</oboInOwl:id>
        <rdfs:label>Huhu Rural Local-Level Government Area</rdfs:label>
    </owl:NamedIndividual>
    


    <!-- http://purl.obolibrary.org/obo/GAZ_00118035 -->

    <owl:NamedIndividual rdf:about="http://purl.obolibrary.org/obo/GAZ_00118035">
        <obo:RO_0001025 rdf:resource="http://purl.obolibrary.org/obo/GAZ_00022381"/>
        <obo:IAO_0000115>A Local-Level Government Area of Alotau District.</obo:IAO_0000115>
        <oboInOwl:hasOBONamespace>GAZ</oboInOwl:hasOBONamespace>
        <oboInOwl:id>GAZ:00118035</oboInOwl:id>
        <rdfs:label>Suau Rural Local-Level Government Area</rdfs:label>
    </owl:NamedIndividual>
    


    <!-- http://purl.obolibrary.org/obo/GAZ_00118036 -->

    <owl:NamedIndividual rdf:about="http://purl.obolibrary.org/obo/GAZ_00118036">
        <obo:RO_0001025 rdf:resource="http://purl.obolibrary.org/obo/GAZ_00022381"/>
        <obo:IAO_0000115>A Local-Level Government Area of Alotau District.</obo:IAO_0000115>
        <oboInOwl:hasOBONamespace>GAZ</oboInOwl:hasOBONamespace>
        <oboInOwl:id>GAZ:00118036</oboInOwl:id>
        <rdfs:label>Alotau Urban Local-Level Government Area</rdfs:label>
    </owl:NamedIndividual>
    


    <!-- http://purl.obolibrary.org/obo/GAZ_00118037 -->

    <owl:NamedIndividual rdf:about="http://purl.obolibrary.org/obo/GAZ_00118037">
        <obo:RO_0001025 rdf:resource="http://purl.obolibrary.org/obo/GAZ_00022380"/>
        <obo:IAO_0000115>A Local-Level Government Area of Esa&apos;ala District.</obo:IAO_0000115>
        <oboInOwl:hasOBONamespace>GAZ</oboInOwl:hasOBONamespace>
        <oboInOwl:id>GAZ:00118037</oboInOwl:id>
        <rdfs:label>Dobu Rural Local-Level Government Area</rdfs:label>
    </owl:NamedIndividual>
    


    <!-- http://purl.obolibrary.org/obo/GAZ_00118038 -->

    <owl:NamedIndividual rdf:about="http://purl.obolibrary.org/obo/GAZ_00118038">
        <obo:RO_0001025 rdf:resource="http://purl.obolibrary.org/obo/GAZ_00022380"/>
        <obo:IAO_0000115>A Local-Level Government Area of Esa&apos;ala District.</obo:IAO_0000115>
        <oboInOwl:hasOBONamespace>GAZ</oboInOwl:hasOBONamespace>
        <oboInOwl:id>GAZ:00118038</oboInOwl:id>
        <rdfs:label>Duau Rural Local-Level Government Area</rdfs:label>
    </owl:NamedIndividual>
    


    <!-- http://purl.obolibrary.org/obo/GAZ_00118039 -->

    <owl:NamedIndividual rdf:about="http://purl.obolibrary.org/obo/GAZ_00118039">
        <obo:RO_0001025 rdf:resource="http://purl.obolibrary.org/obo/GAZ_00022380"/>
        <obo:IAO_0000115>A Local-Level Government Area of Esa&apos;ala District.</obo:IAO_0000115>
        <oboInOwl:hasOBONamespace>GAZ</oboInOwl:hasOBONamespace>
        <oboInOwl:id>GAZ:00118039</oboInOwl:id>
        <rdfs:label>West Ferguson Local-Level Government Area</rdfs:label>
    </owl:NamedIndividual>
    


    <!-- http://purl.obolibrary.org/obo/GAZ_00118040 -->

    <owl:NamedIndividual rdf:about="http://purl.obolibrary.org/obo/GAZ_00118040">
        <obo:RO_0001025 rdf:resource="http://purl.obolibrary.org/obo/GAZ_00022382"/>
        <obo:IAO_0000115>A Local-Level Government Area of Kiriwini-Goodenough District.</obo:IAO_0000115>
        <oboInOwl:hasOBONamespace>GAZ</oboInOwl:hasOBONamespace>
        <oboInOwl:id>GAZ:00118040</oboInOwl:id>
        <rdfs:label>Goodenough Island Rural Local-Level Government Area</rdfs:label>
    </owl:NamedIndividual>
    


    <!-- http://purl.obolibrary.org/obo/GAZ_00118041 -->

    <owl:NamedIndividual rdf:about="http://purl.obolibrary.org/obo/GAZ_00118041">
        <obo:RO_0001025 rdf:resource="http://purl.obolibrary.org/obo/GAZ_00022382"/>
        <obo:IAO_0000115>A Local-Level Government Area of Kiriwini-Goodenough District.</obo:IAO_0000115>
        <oboInOwl:hasOBONamespace>GAZ</oboInOwl:hasOBONamespace>
        <oboInOwl:id>GAZ:00118041</oboInOwl:id>
        <rdfs:label>Kiriwini Rural Local-Level Government Area</rdfs:label>
    </owl:NamedIndividual>
    


    <!-- http://purl.obolibrary.org/obo/GAZ_00118042 -->

    <owl:NamedIndividual rdf:about="http://purl.obolibrary.org/obo/GAZ_00118042">
        <obo:RO_0001025 rdf:resource="http://purl.obolibrary.org/obo/GAZ_00022379"/>
        <obo:IAO_0000115>A Local-Level Government Area of Samarai-Murua District.</obo:IAO_0000115>
        <oboInOwl:hasOBONamespace>GAZ</oboInOwl:hasOBONamespace>
        <oboInOwl:id>GAZ:00118042</oboInOwl:id>
        <rdfs:label>Bwanabwana Rural Local-Level Government Area</rdfs:label>
    </owl:NamedIndividual>
    


    <!-- http://purl.obolibrary.org/obo/GAZ_00118043 -->

    <owl:NamedIndividual rdf:about="http://purl.obolibrary.org/obo/GAZ_00118043">
        <obo:RO_0001025 rdf:resource="http://purl.obolibrary.org/obo/GAZ_00022379"/>
        <obo:IAO_0000115>A Local-Level Government Area of Samarai-Murua District.</obo:IAO_0000115>
        <oboInOwl:hasOBONamespace>GAZ</oboInOwl:hasOBONamespace>
        <oboInOwl:id>GAZ:00118043</oboInOwl:id>
        <rdfs:label>Yaleyamba Rural Local-Level Government Area</rdfs:label>
    </owl:NamedIndividual>
    


    <!-- http://purl.obolibrary.org/obo/GAZ_00118044 -->

    <owl:NamedIndividual rdf:about="http://purl.obolibrary.org/obo/GAZ_00118044">
        <obo:RO_0001025 rdf:resource="http://purl.obolibrary.org/obo/GAZ_00022379"/>
        <obo:IAO_0000115>A Local-Level Government Area of Samarai-Murua District.</obo:IAO_0000115>
        <oboInOwl:hasOBONamespace>GAZ</oboInOwl:hasOBONamespace>
        <oboInOwl:id>GAZ:00118044</oboInOwl:id>
        <rdfs:label>Murua Rural Local-Level Government Area</rdfs:label>
    </owl:NamedIndividual>
    


    <!-- http://purl.obolibrary.org/obo/GAZ_00118045 -->

    <owl:NamedIndividual rdf:about="http://purl.obolibrary.org/obo/GAZ_00118045">
        <obo:RO_0001025 rdf:resource="http://purl.obolibrary.org/obo/GAZ_00022379"/>
        <obo:IAO_0000115>A Local-Level Government Area of Samarai-Murua District.</obo:IAO_0000115>
        <oboInOwl:hasOBONamespace>GAZ</oboInOwl:hasOBONamespace>
        <oboInOwl:id>GAZ:00118045</oboInOwl:id>
        <rdfs:label>Louisade Rural Local-Level Government Area</rdfs:label>
    </owl:NamedIndividual>
    


    <!-- http://purl.obolibrary.org/obo/GAZ_00118046 -->

    <owl:NamedIndividual rdf:about="http://purl.obolibrary.org/obo/GAZ_00118046">
        <obo:RO_0001025 rdf:resource="http://purl.obolibrary.org/obo/GAZ_00022409"/>
        <obo:IAO_0000115>A Local-Level Government Area of Ijivitari District.</obo:IAO_0000115>
        <oboInOwl:hasOBONamespace>GAZ</oboInOwl:hasOBONamespace>
        <oboInOwl:id>GAZ:00118046</oboInOwl:id>
        <rdfs:label>Afore Rural Local-Level Government Area</rdfs:label>
    </owl:NamedIndividual>
    


    <!-- http://purl.obolibrary.org/obo/GAZ_00118047 -->

    <owl:NamedIndividual rdf:about="http://purl.obolibrary.org/obo/GAZ_00118047">
        <obo:RO_0001025 rdf:resource="http://purl.obolibrary.org/obo/GAZ_00022409"/>
        <obo:IAO_0000115>A Local-Level Government Area of Ijivitari District.</obo:IAO_0000115>
        <oboInOwl:hasOBONamespace>GAZ</oboInOwl:hasOBONamespace>
        <oboInOwl:id>GAZ:00118047</oboInOwl:id>
        <rdfs:label>Cape Nelson Rural Local-Level Government Area</rdfs:label>
    </owl:NamedIndividual>
    


    <!-- http://purl.obolibrary.org/obo/GAZ_00118048 -->

    <owl:NamedIndividual rdf:about="http://purl.obolibrary.org/obo/GAZ_00118048">
        <obo:RO_0001025 rdf:resource="http://purl.obolibrary.org/obo/GAZ_00022409"/>
        <obo:IAO_0000115>A Local-Level Government Area of Ijivitari District.</obo:IAO_0000115>
        <oboInOwl:hasOBONamespace>GAZ</oboInOwl:hasOBONamespace>
        <oboInOwl:id>GAZ:00118048</oboInOwl:id>
        <rdfs:label>Oro Bay Rural Local-Level Government Area</rdfs:label>
    </owl:NamedIndividual>
    


    <!-- http://purl.obolibrary.org/obo/GAZ_00118049 -->

    <owl:NamedIndividual rdf:about="http://purl.obolibrary.org/obo/GAZ_00118049">
        <obo:RO_0001025 rdf:resource="http://purl.obolibrary.org/obo/GAZ_00022409"/>
        <obo:IAO_0000115>A Local-Level Government Area of Ijivitari District.</obo:IAO_0000115>
        <oboInOwl:hasOBONamespace>GAZ</oboInOwl:hasOBONamespace>
        <oboInOwl:id>GAZ:00118049</oboInOwl:id>
        <rdfs:label>Popendetta Urban Local-Level Government Area</rdfs:label>
    </owl:NamedIndividual>
    


    <!-- http://purl.obolibrary.org/obo/GAZ_00118050 -->

    <owl:NamedIndividual rdf:about="http://purl.obolibrary.org/obo/GAZ_00118050">
        <obo:RO_0001025 rdf:resource="http://purl.obolibrary.org/obo/GAZ_00022410"/>
        <obo:IAO_0000115>A Local-Level Government Area of Sohe District.</obo:IAO_0000115>
        <oboInOwl:hasOBONamespace>GAZ</oboInOwl:hasOBONamespace>
        <oboInOwl:id>GAZ:00118050</oboInOwl:id>
        <rdfs:label>Kira Rural Local-Level Government Area</rdfs:label>
    </owl:NamedIndividual>
    


    <!-- http://purl.obolibrary.org/obo/GAZ_00118051 -->

    <owl:NamedIndividual rdf:about="http://purl.obolibrary.org/obo/GAZ_00118051">
        <obo:RO_0001025 rdf:resource="http://purl.obolibrary.org/obo/GAZ_00022410"/>
        <obo:IAO_0000115>A Local-Level Government Area of Sohe District.</obo:IAO_0000115>
        <oboInOwl:hasOBONamespace>GAZ</oboInOwl:hasOBONamespace>
        <oboInOwl:id>GAZ:00118051</oboInOwl:id>
        <rdfs:label>Tamata Rural Local-Level Government Area</rdfs:label>
    </owl:NamedIndividual>
    


    <!-- http://purl.obolibrary.org/obo/GAZ_00118052 -->

    <owl:NamedIndividual rdf:about="http://purl.obolibrary.org/obo/GAZ_00118052">
        <obo:RO_0001025 rdf:resource="http://purl.obolibrary.org/obo/GAZ_00022410"/>
        <obo:IAO_0000115>A Local-Level Government Area of Sohe District.</obo:IAO_0000115>
        <oboInOwl:hasOBONamespace>GAZ</oboInOwl:hasOBONamespace>
        <oboInOwl:id>GAZ:00118052</oboInOwl:id>
        <rdfs:label>Kokoda Rural Local-Level Government Area</rdfs:label>
    </owl:NamedIndividual>
    


    <!-- http://purl.obolibrary.org/obo/GAZ_00118053 -->

    <owl:NamedIndividual rdf:about="http://purl.obolibrary.org/obo/GAZ_00118053">
        <obo:RO_0001025 rdf:resource="http://purl.obolibrary.org/obo/GAZ_00022410"/>
        <obo:IAO_0000115>A Local-Level Government Area of Sohe District.</obo:IAO_0000115>
        <oboInOwl:hasOBONamespace>GAZ</oboInOwl:hasOBONamespace>
        <oboInOwl:id>GAZ:00118053</oboInOwl:id>
        <rdfs:label>Higaturu Rural Local-Level Government Area</rdfs:label>
    </owl:NamedIndividual>
    


    <!-- http://purl.obolibrary.org/obo/GAZ_00118054 -->

    <owl:NamedIndividual rdf:about="http://purl.obolibrary.org/obo/GAZ_00118054">
        <obo:RO_0001025 rdf:resource="http://purl.obolibrary.org/obo/GAZ_00022418"/>
        <obo:IAO_0000115>An island in the Western Province of Papua New Guinea, the town on the island goes by the same name and is the capital of the Province. It is located near the mouth of the Fly River on the western side of the Gulf, just north of Torres Strait and Far North Queensland.</obo:IAO_0000115>
        <oboInOwl:hasOBONamespace>GAZ</oboInOwl:hasOBONamespace>
        <oboInOwl:id>GAZ:00118054</oboInOwl:id>
        <rdfs:label>Daru Island</rdfs:label>
    </owl:NamedIndividual>
    


    <!-- http://purl.obolibrary.org/obo/GAZ_00118055 -->

    <owl:NamedIndividual rdf:about="http://purl.obolibrary.org/obo/GAZ_00118055">
        <obo:RO_0001025 rdf:resource="http://purl.obolibrary.org/obo/GAZ_00022417"/>
        <obo:IAO_0000115>A Local-Level Government Area of North Fly District.</obo:IAO_0000115>
        <oboInOwl:hasOBONamespace>GAZ</oboInOwl:hasOBONamespace>
        <oboInOwl:id>GAZ:00118055</oboInOwl:id>
        <rdfs:label>Star Mountains Rural Local-Level Government Area</rdfs:label>
    </owl:NamedIndividual>
    


    <!-- http://purl.obolibrary.org/obo/GAZ_00118056 -->

    <owl:NamedIndividual rdf:about="http://purl.obolibrary.org/obo/GAZ_00118056">
        <obo:RO_0001025 rdf:resource="http://purl.obolibrary.org/obo/GAZ_00022417"/>
        <obo:IAO_0000115>A Local-Level Government Area of North Fly District.</obo:IAO_0000115>
        <oboInOwl:hasOBONamespace>GAZ</oboInOwl:hasOBONamespace>
        <oboInOwl:id>GAZ:00118056</oboInOwl:id>
        <rdfs:label>Olsobip Rural Local-Level Government Area</rdfs:label>
    </owl:NamedIndividual>
    


    <!-- http://purl.obolibrary.org/obo/GAZ_00118057 -->

    <owl:NamedIndividual rdf:about="http://purl.obolibrary.org/obo/GAZ_00118057">
        <obo:RO_0001025 rdf:resource="http://purl.obolibrary.org/obo/GAZ_00022417"/>
        <obo:IAO_0000115>A Local-Level Government Area of North Fly District.</obo:IAO_0000115>
        <oboInOwl:hasOBONamespace>GAZ</oboInOwl:hasOBONamespace>
        <oboInOwl:id>GAZ:00118057</oboInOwl:id>
        <rdfs:label>Kiunga Rural Local-Level Government Area</rdfs:label>
    </owl:NamedIndividual>
    


    <!-- http://purl.obolibrary.org/obo/GAZ_00118058 -->

    <owl:NamedIndividual rdf:about="http://purl.obolibrary.org/obo/GAZ_00118058">
        <obo:RO_0001025 rdf:resource="http://purl.obolibrary.org/obo/GAZ_00022417"/>
        <obo:IAO_0000115>A Local-Level Government Area of North Fly District.</obo:IAO_0000115>
        <oboInOwl:hasOBONamespace>GAZ</oboInOwl:hasOBONamespace>
        <oboInOwl:id>GAZ:00118058</oboInOwl:id>
        <rdfs:label>Ningerum Rural Local-Level Government Area</rdfs:label>
    </owl:NamedIndividual>
    


    <!-- http://purl.obolibrary.org/obo/GAZ_00118059 -->

    <owl:NamedIndividual rdf:about="http://purl.obolibrary.org/obo/GAZ_00118059">
        <obo:RO_0001025 rdf:resource="http://purl.obolibrary.org/obo/GAZ_00022417"/>
        <obo:IAO_0000115>A Local-Level Government Area of North Fly District.</obo:IAO_0000115>
        <oboInOwl:hasOBONamespace>GAZ</oboInOwl:hasOBONamespace>
        <oboInOwl:id>GAZ:00118059</oboInOwl:id>
        <rdfs:label>Kiunga Urban Local-Level Government Area</rdfs:label>
    </owl:NamedIndividual>
    


    <!-- http://purl.obolibrary.org/obo/GAZ_00118060 -->

    <owl:NamedIndividual rdf:about="http://purl.obolibrary.org/obo/GAZ_00118060">
        <obo:RO_0001025 rdf:resource="http://purl.obolibrary.org/obo/GAZ_00022419"/>
        <obo:IAO_0000115>A Local-Level Government Area of Middle Fly District.</obo:IAO_0000115>
        <oboInOwl:hasOBONamespace>GAZ</oboInOwl:hasOBONamespace>
        <oboInOwl:id>GAZ:00118060</oboInOwl:id>
        <rdfs:label>Nomad Rural Local-Level Government Area</rdfs:label>
    </owl:NamedIndividual>
    


    <!-- http://purl.obolibrary.org/obo/GAZ_00118061 -->

    <owl:NamedIndividual rdf:about="http://purl.obolibrary.org/obo/GAZ_00118061">
        <obo:RO_0001025 rdf:resource="http://purl.obolibrary.org/obo/GAZ_00022419"/>
        <obo:IAO_0000115>A Local-Level Government Area of Middle Fly District.</obo:IAO_0000115>
        <oboInOwl:hasOBONamespace>GAZ</oboInOwl:hasOBONamespace>
        <oboInOwl:id>GAZ:00118061</oboInOwl:id>
        <rdfs:label>Lake Murray Rural Local-Level Government Area</rdfs:label>
    </owl:NamedIndividual>
    


    <!-- http://purl.obolibrary.org/obo/GAZ_00118062 -->

    <owl:NamedIndividual rdf:about="http://purl.obolibrary.org/obo/GAZ_00118062">
        <obo:RO_0001025 rdf:resource="http://purl.obolibrary.org/obo/GAZ_00022419"/>
        <obo:IAO_0000115>A Local-Level Government Area of Middle Fly District.</obo:IAO_0000115>
        <oboInOwl:hasOBONamespace>GAZ</oboInOwl:hasOBONamespace>
        <oboInOwl:id>GAZ:00118062</oboInOwl:id>
        <rdfs:label>Gogodala Rural Local-Level Government Area</rdfs:label>
    </owl:NamedIndividual>
    


    <!-- http://purl.obolibrary.org/obo/GAZ_00118063 -->

    <owl:NamedIndividual rdf:about="http://purl.obolibrary.org/obo/GAZ_00118063">
        <obo:RO_0001025 rdf:resource="http://purl.obolibrary.org/obo/GAZ_00022419"/>
        <obo:IAO_0000115>A Local-Level Government Area of Middle Fly District.</obo:IAO_0000115>
        <oboInOwl:hasOBONamespace>GAZ</oboInOwl:hasOBONamespace>
        <oboInOwl:id>GAZ:00118063</oboInOwl:id>
        <rdfs:label>Bamu Rural Local-Level Government Area</rdfs:label>
    </owl:NamedIndividual>
    


    <!-- http://purl.obolibrary.org/obo/GAZ_00118064 -->

    <owl:NamedIndividual rdf:about="http://purl.obolibrary.org/obo/GAZ_00118064">
        <obo:RO_0001025 rdf:resource="http://purl.obolibrary.org/obo/GAZ_00022419"/>
        <obo:IAO_0000115>A Local-Level Government Area of Middle Fly District.</obo:IAO_0000115>
        <oboInOwl:hasOBONamespace>GAZ</oboInOwl:hasOBONamespace>
        <oboInOwl:id>GAZ:00118064</oboInOwl:id>
        <rdfs:label>Balimo Urban Local-Level Government Area</rdfs:label>
    </owl:NamedIndividual>
    


    <!-- http://purl.obolibrary.org/obo/GAZ_00118065 -->

    <owl:NamedIndividual rdf:about="http://purl.obolibrary.org/obo/GAZ_00118065">
        <obo:RO_0001025 rdf:resource="http://purl.obolibrary.org/obo/GAZ_00118054"/>
        <obo:IAO_0000115>A Local-Level Government Area of South Fly District.</obo:IAO_0000115>
        <oboInOwl:hasOBONamespace>GAZ</oboInOwl:hasOBONamespace>
        <oboInOwl:id>GAZ:00118065</oboInOwl:id>
        <rdfs:label>Daru Urban Local-Level Government Area</rdfs:label>
    </owl:NamedIndividual>
    


    <!-- http://purl.obolibrary.org/obo/GAZ_00118066 -->

    <owl:NamedIndividual rdf:about="http://purl.obolibrary.org/obo/GAZ_00118066">
        <obo:RO_0001025 rdf:resource="http://purl.obolibrary.org/obo/GAZ_00022418"/>
        <obo:IAO_0000115>A Local-Level Government Area of South Fly District.</obo:IAO_0000115>
        <oboInOwl:hasOBONamespace>GAZ</oboInOwl:hasOBONamespace>
        <oboInOwl:id>GAZ:00118066</oboInOwl:id>
        <rdfs:label>Oriomo-Bituri Rural Local-Level Government Area</rdfs:label>
    </owl:NamedIndividual>
    


    <!-- http://purl.obolibrary.org/obo/GAZ_00118067 -->

    <owl:NamedIndividual rdf:about="http://purl.obolibrary.org/obo/GAZ_00118067">
        <obo:RO_0001025 rdf:resource="http://purl.obolibrary.org/obo/GAZ_00022418"/>
        <obo:IAO_0000115>A Local-Level Government Area of South Fly District.</obo:IAO_0000115>
        <oboInOwl:hasOBONamespace>GAZ</oboInOwl:hasOBONamespace>
        <oboInOwl:id>GAZ:00118067</oboInOwl:id>
        <rdfs:label>Kiwai Rural Local-Level Government Area</rdfs:label>
    </owl:NamedIndividual>
    


    <!-- http://purl.obolibrary.org/obo/GAZ_00118068 -->

    <owl:NamedIndividual rdf:about="http://purl.obolibrary.org/obo/GAZ_00118068">
        <obo:RO_0001025 rdf:resource="http://purl.obolibrary.org/obo/GAZ_00022418"/>
        <obo:IAO_0000115>A Local-Level Government Area of South Fly District.</obo:IAO_0000115>
        <oboInOwl:hasOBONamespace>GAZ</oboInOwl:hasOBONamespace>
        <oboInOwl:id>GAZ:00118068</oboInOwl:id>
        <rdfs:label>Morehead Rural Local-Level Government Area</rdfs:label>
    </owl:NamedIndividual>
    


    <!-- http://purl.obolibrary.org/obo/GAZ_00118069 -->

    <owl:NamedIndividual rdf:about="http://purl.obolibrary.org/obo/GAZ_00118069">
        <obo:RO_0001025 rdf:resource="http://purl.obolibrary.org/obo/GAZ_00022345"/>
        <obo:IAO_0000115>A Local-Level Government Area of Pomio District.</obo:IAO_0000115>
        <oboInOwl:hasOBONamespace>GAZ</oboInOwl:hasOBONamespace>
        <oboInOwl:id>GAZ:00118069</oboInOwl:id>
        <rdfs:label>Central-Inland Pomio Rural Local-Level Government Area</rdfs:label>
    </owl:NamedIndividual>
    


    <!-- http://purl.obolibrary.org/obo/GAZ_00118070 -->

    <owl:NamedIndividual rdf:about="http://purl.obolibrary.org/obo/GAZ_00118070">
        <obo:RO_0001025 rdf:resource="http://purl.obolibrary.org/obo/GAZ_00022345"/>
        <obo:IAO_0000115>A Local-Level Government Area of Pomio District.</obo:IAO_0000115>
        <oboInOwl:hasOBONamespace>GAZ</oboInOwl:hasOBONamespace>
        <oboInOwl:id>GAZ:00118070</oboInOwl:id>
        <rdfs:label>Melkoi Rural Local-Level Government Area</rdfs:label>
    </owl:NamedIndividual>
    


    <!-- http://purl.obolibrary.org/obo/GAZ_00118071 -->

    <owl:NamedIndividual rdf:about="http://purl.obolibrary.org/obo/GAZ_00118071">
        <obo:RO_0001025 rdf:resource="http://purl.obolibrary.org/obo/GAZ_00022345"/>
        <obo:IAO_0000115>A Local-Level Government Area of Pomio District.</obo:IAO_0000115>
        <oboInOwl:hasOBONamespace>GAZ</oboInOwl:hasOBONamespace>
        <oboInOwl:id>GAZ:00118071</oboInOwl:id>
        <rdfs:label>Sinivit Rural Local-Level Government Area</rdfs:label>
    </owl:NamedIndividual>
    


    <!-- http://purl.obolibrary.org/obo/GAZ_00118072 -->

    <owl:NamedIndividual rdf:about="http://purl.obolibrary.org/obo/GAZ_00118072">
        <obo:RO_0001025 rdf:resource="http://purl.obolibrary.org/obo/GAZ_00022345"/>
        <obo:IAO_0000115>A Local-Level Government Area of Pomio District.</obo:IAO_0000115>
        <oboInOwl:hasOBONamespace>GAZ</oboInOwl:hasOBONamespace>
        <oboInOwl:id>GAZ:00118072</oboInOwl:id>
        <rdfs:label>East Pomio Rural Local-Level Government Area</rdfs:label>
    </owl:NamedIndividual>
    


    <!-- http://purl.obolibrary.org/obo/GAZ_00118073 -->

    <owl:NamedIndividual rdf:about="http://purl.obolibrary.org/obo/GAZ_00118073">
        <obo:RO_0001025 rdf:resource="http://purl.obolibrary.org/obo/GAZ_00022345"/>
        <obo:IAO_0000115>A Local-Level Government Area of Pomio District.</obo:IAO_0000115>
        <oboInOwl:hasOBONamespace>GAZ</oboInOwl:hasOBONamespace>
        <oboInOwl:id>GAZ:00118073</oboInOwl:id>
        <rdfs:label>West Pomio-Mamusi Rural Local-Level Government Area</rdfs:label>
    </owl:NamedIndividual>
    


    <!-- http://purl.obolibrary.org/obo/GAZ_00118074 -->

    <owl:NamedIndividual rdf:about="http://purl.obolibrary.org/obo/GAZ_00118074">
        <obo:RO_0001025 rdf:resource="http://purl.obolibrary.org/obo/GAZ_00022347"/>
        <obo:IAO_0000115>A Local-Level Government Area of Kokopo District.</obo:IAO_0000115>
        <oboInOwl:hasOBONamespace>GAZ</oboInOwl:hasOBONamespace>
        <oboInOwl:id>GAZ:00118074</oboInOwl:id>
        <rdfs:label>Bitapaka Rural Local-Level Government Area</rdfs:label>
    </owl:NamedIndividual>
    


    <!-- http://purl.obolibrary.org/obo/GAZ_00118075 -->

    <owl:NamedIndividual rdf:about="http://purl.obolibrary.org/obo/GAZ_00118075">
        <obo:RO_0001025 rdf:resource="http://purl.obolibrary.org/obo/GAZ_00022347"/>
        <obo:IAO_0000115>A Local-Level Government Area of Kokopo District.</obo:IAO_0000115>
        <oboInOwl:hasOBONamespace>GAZ</oboInOwl:hasOBONamespace>
        <oboInOwl:id>GAZ:00118075</oboInOwl:id>
        <rdfs:label>Duke of York Rural Local-Level Government Area</rdfs:label>
    </owl:NamedIndividual>
    


    <!-- http://purl.obolibrary.org/obo/GAZ_00118076 -->

    <owl:NamedIndividual rdf:about="http://purl.obolibrary.org/obo/GAZ_00118076">
        <obo:RO_0001025 rdf:resource="http://purl.obolibrary.org/obo/GAZ_00022347"/>
        <obo:IAO_0000115>A Local-Level Government Area of Kokopo District.</obo:IAO_0000115>
        <oboInOwl:hasOBONamespace>GAZ</oboInOwl:hasOBONamespace>
        <oboInOwl:id>GAZ:00118076</oboInOwl:id>
        <rdfs:label>Kokopo-Vunamami Urban Local-Level Government Area</rdfs:label>
    </owl:NamedIndividual>
    


    <!-- http://purl.obolibrary.org/obo/GAZ_00118077 -->

    <owl:NamedIndividual rdf:about="http://purl.obolibrary.org/obo/GAZ_00118077">
        <obo:RO_0001025 rdf:resource="http://purl.obolibrary.org/obo/GAZ_00022347"/>
        <obo:IAO_0000115>A Local-Level Government Area of Kokopo District.</obo:IAO_0000115>
        <oboInOwl:hasOBONamespace>GAZ</oboInOwl:hasOBONamespace>
        <oboInOwl:id>GAZ:00118077</oboInOwl:id>
        <rdfs:label>Raluana Rural Local-Level Government Area</rdfs:label>
    </owl:NamedIndividual>
    


    <!-- http://purl.obolibrary.org/obo/GAZ_00118078 -->

    <owl:NamedIndividual rdf:about="http://purl.obolibrary.org/obo/GAZ_00118078">
        <obo:RO_0001025 rdf:resource="http://purl.obolibrary.org/obo/GAZ_00022348"/>
        <obo:IAO_0000115>A Local-Level Government Area of Gazelle District.</obo:IAO_0000115>
        <oboInOwl:hasOBONamespace>GAZ</oboInOwl:hasOBONamespace>
        <oboInOwl:id>GAZ:00118078</oboInOwl:id>
        <rdfs:label>Lassul Baining Rural Local-Level Government Area</rdfs:label>
    </owl:NamedIndividual>
    


    <!-- http://purl.obolibrary.org/obo/GAZ_00118079 -->

    <owl:NamedIndividual rdf:about="http://purl.obolibrary.org/obo/GAZ_00118079">
        <obo:RO_0001025 rdf:resource="http://purl.obolibrary.org/obo/GAZ_00022348"/>
        <obo:IAO_0000115>A Local-Level Government Area of Gazelle District.</obo:IAO_0000115>
        <oboInOwl:hasOBONamespace>GAZ</oboInOwl:hasOBONamespace>
        <oboInOwl:id>GAZ:00118079</oboInOwl:id>
        <rdfs:label>Inland Baining Rural Local-Level Government Area</rdfs:label>
    </owl:NamedIndividual>
    


    <!-- http://purl.obolibrary.org/obo/GAZ_00118080 -->

    <owl:NamedIndividual rdf:about="http://purl.obolibrary.org/obo/GAZ_00118080">
        <obo:RO_0001025 rdf:resource="http://purl.obolibrary.org/obo/GAZ_00022348"/>
        <obo:IAO_0000115>A Local-Level Government Area of Gazelle District.</obo:IAO_0000115>
        <oboInOwl:hasOBONamespace>GAZ</oboInOwl:hasOBONamespace>
        <oboInOwl:id>GAZ:00118080</oboInOwl:id>
        <rdfs:label>Toma-Vunadidir Rural Local-Level Government Area</rdfs:label>
    </owl:NamedIndividual>
    


    <!-- http://purl.obolibrary.org/obo/GAZ_00118081 -->

    <owl:NamedIndividual rdf:about="http://purl.obolibrary.org/obo/GAZ_00118081">
        <obo:RO_0001025 rdf:resource="http://purl.obolibrary.org/obo/GAZ_00022348"/>
        <obo:IAO_0000115>A Local-Level Government Area of Gazelle District.</obo:IAO_0000115>
        <oboInOwl:hasOBONamespace>GAZ</oboInOwl:hasOBONamespace>
        <oboInOwl:id>GAZ:00118081</oboInOwl:id>
        <rdfs:label>Livuan-Reimber Rural Local-Level Government Area</rdfs:label>
    </owl:NamedIndividual>
    


    <!-- http://purl.obolibrary.org/obo/GAZ_00118082 -->

    <owl:NamedIndividual rdf:about="http://purl.obolibrary.org/obo/GAZ_00118082">
        <obo:RO_0001025 rdf:resource="http://purl.obolibrary.org/obo/GAZ_00022348"/>
        <obo:IAO_0000115>A Local-Level Government Area of Gazelle District.</obo:IAO_0000115>
        <oboInOwl:hasOBONamespace>GAZ</oboInOwl:hasOBONamespace>
        <oboInOwl:id>GAZ:00118082</oboInOwl:id>
        <rdfs:label>Central Gazelle Rural Local-Level Government Area</rdfs:label>
    </owl:NamedIndividual>
    


    <!-- http://purl.obolibrary.org/obo/GAZ_00118083 -->

    <owl:NamedIndividual rdf:about="http://purl.obolibrary.org/obo/GAZ_00118083">
        <obo:RO_0001025 rdf:resource="http://purl.obolibrary.org/obo/GAZ_00022378"/>
        <obo:IAO_0000115>A Local-Level Government Area of Manus District.</obo:IAO_0000115>
        <oboInOwl:hasOBONamespace>GAZ</oboInOwl:hasOBONamespace>
        <oboInOwl:id>GAZ:00118083</oboInOwl:id>
        <rdfs:label>Bisikani-Soparibeu Kabin Rural Local-Level Government Area</rdfs:label>
    </owl:NamedIndividual>
    


    <!-- http://purl.obolibrary.org/obo/GAZ_00118084 -->

    <owl:NamedIndividual rdf:about="http://purl.obolibrary.org/obo/GAZ_00118084">
        <obo:RO_0001025 rdf:resource="http://purl.obolibrary.org/obo/GAZ_00022378"/>
        <obo:IAO_0000115>A Local-Level Government Area of Manus District.</obo:IAO_0000115>
        <oboInOwl:hasOBONamespace>GAZ</oboInOwl:hasOBONamespace>
        <oboInOwl:id>GAZ:00118084</oboInOwl:id>
        <rdfs:label>Tetidu Rural Local-Level Government Area</rdfs:label>
    </owl:NamedIndividual>
    


    <!-- http://purl.obolibrary.org/obo/GAZ_00118085 -->

    <owl:NamedIndividual rdf:about="http://purl.obolibrary.org/obo/GAZ_00118085">
        <obo:RO_0001025 rdf:resource="http://purl.obolibrary.org/obo/GAZ_00022378"/>
        <obo:IAO_0000115>A Local-Level Government Area of Manus District.</obo:IAO_0000115>
        <oboInOwl:hasOBONamespace>GAZ</oboInOwl:hasOBONamespace>
        <oboInOwl:id>GAZ:00118085</oboInOwl:id>
        <rdfs:label>Pomutu-Kurti-Andra Rural Local-Level Government Area</rdfs:label>
    </owl:NamedIndividual>
    


    <!-- http://purl.obolibrary.org/obo/GAZ_00118086 -->

    <owl:NamedIndividual rdf:about="http://purl.obolibrary.org/obo/GAZ_00118086">
        <obo:RO_0001025 rdf:resource="http://purl.obolibrary.org/obo/GAZ_00022378"/>
        <obo:IAO_0000115>A Local-Level Government Area of Manus District.</obo:IAO_0000115>
        <oboInOwl:hasOBONamespace>GAZ</oboInOwl:hasOBONamespace>
        <oboInOwl:id>GAZ:00118086</oboInOwl:id>
        <rdfs:label>Lorengau Urban Local-Level Government Area</rdfs:label>
    </owl:NamedIndividual>
    


    <!-- http://purl.obolibrary.org/obo/GAZ_00118087 -->

    <owl:NamedIndividual rdf:about="http://purl.obolibrary.org/obo/GAZ_00118087">
        <obo:RO_0001025 rdf:resource="http://purl.obolibrary.org/obo/GAZ_00022378"/>
        <obo:IAO_0000115>A Local-Level Government Area of Manus District.</obo:IAO_0000115>
        <oboInOwl:hasOBONamespace>GAZ</oboInOwl:hasOBONamespace>
        <oboInOwl:id>GAZ:00118087</oboInOwl:id>
        <rdfs:label>Balopa Rural Local-Level Government Area</rdfs:label>
    </owl:NamedIndividual>
    


    <!-- http://purl.obolibrary.org/obo/GAZ_00118088 -->

    <owl:NamedIndividual rdf:about="http://purl.obolibrary.org/obo/GAZ_00118088">
        <obo:RO_0001025 rdf:resource="http://purl.obolibrary.org/obo/GAZ_00022378"/>
        <obo:IAO_0000115>A Local-Level Government Area of Manus District.</obo:IAO_0000115>
        <oboInOwl:hasOBONamespace>GAZ</oboInOwl:hasOBONamespace>
        <oboInOwl:id>GAZ:00118088</oboInOwl:id>
        <rdfs:label>Nigoherm Rural Local-Level Government Area</rdfs:label>
    </owl:NamedIndividual>
    


    <!-- http://purl.obolibrary.org/obo/GAZ_00118089 -->

    <owl:NamedIndividual rdf:about="http://purl.obolibrary.org/obo/GAZ_00118089">
        <obo:RO_0001025 rdf:resource="http://purl.obolibrary.org/obo/GAZ_00022378"/>
        <obo:IAO_0000115>A Local-Level Government Area of Manus District.</obo:IAO_0000115>
        <oboInOwl:hasOBONamespace>GAZ</oboInOwl:hasOBONamespace>
        <oboInOwl:id>GAZ:00118089</oboInOwl:id>
        <rdfs:label>Rapatona Rural Local-Level Government Area</rdfs:label>
    </owl:NamedIndividual>
    


    <!-- http://purl.obolibrary.org/obo/GAZ_00118090 -->

    <owl:NamedIndividual rdf:about="http://purl.obolibrary.org/obo/GAZ_00118090">
        <obo:RO_0001025 rdf:resource="http://purl.obolibrary.org/obo/GAZ_00022378"/>
        <obo:IAO_0000115>A Local-Level Government Area of Manus District.</obo:IAO_0000115>
        <oboInOwl:hasOBONamespace>GAZ</oboInOwl:hasOBONamespace>
        <oboInOwl:id>GAZ:00118090</oboInOwl:id>
        <rdfs:label>Los Negros Rural Local-Level Government Area</rdfs:label>
    </owl:NamedIndividual>
    


    <!-- http://purl.obolibrary.org/obo/GAZ_00118091 -->

    <owl:NamedIndividual rdf:about="http://purl.obolibrary.org/obo/GAZ_00118091">
        <obo:RO_0001025 rdf:resource="http://purl.obolibrary.org/obo/GAZ_00022378"/>
        <obo:IAO_0000115>A Local-Level Government Area of Manus District.</obo:IAO_0000115>
        <oboInOwl:hasOBONamespace>GAZ</oboInOwl:hasOBONamespace>
        <oboInOwl:id>GAZ:00118091</oboInOwl:id>
        <rdfs:label>Nali Sopat-Penabu Rural Local-Level Government Area</rdfs:label>
    </owl:NamedIndividual>
    


    <!-- http://purl.obolibrary.org/obo/GAZ_00118092 -->

    <owl:NamedIndividual rdf:about="http://purl.obolibrary.org/obo/GAZ_00118092">
        <obo:RO_0001025 rdf:resource="http://purl.obolibrary.org/obo/GAZ_00022378"/>
        <obo:IAO_0000115>A Local-Level Government Area of Manus District.</obo:IAO_0000115>
        <oboInOwl:hasOBONamespace>GAZ</oboInOwl:hasOBONamespace>
        <oboInOwl:id>GAZ:00118092</oboInOwl:id>
        <rdfs:label>Lelemadih-Bupi Chupei Rural Local-Level Government Area</rdfs:label>
    </owl:NamedIndividual>
    


    <!-- http://purl.obolibrary.org/obo/GAZ_00118093 -->

    <owl:NamedIndividual rdf:about="http://purl.obolibrary.org/obo/GAZ_00118093">
        <obo:RO_0001025 rdf:resource="http://purl.obolibrary.org/obo/GAZ_00022378"/>
        <obo:IAO_0000115>A Local-Level Government Area of Manus District.</obo:IAO_0000115>
        <oboInOwl:hasOBONamespace>GAZ</oboInOwl:hasOBONamespace>
        <oboInOwl:id>GAZ:00118093</oboInOwl:id>
        <rdfs:label>Pobuma Rural Local-Level Government Area</rdfs:label>
    </owl:NamedIndividual>
    


    <!-- http://purl.obolibrary.org/obo/GAZ_00118094 -->

    <owl:NamedIndividual rdf:about="http://purl.obolibrary.org/obo/GAZ_00118094">
        <obo:RO_0001025 rdf:resource="http://purl.obolibrary.org/obo/GAZ_00022378"/>
        <obo:IAO_0000115>A Local-Level Government Area of Manus District.</obo:IAO_0000115>
        <oboInOwl:hasOBONamespace>GAZ</oboInOwl:hasOBONamespace>
        <oboInOwl:id>GAZ:00118094</oboInOwl:id>
        <rdfs:label>Aua-Wuvulu Rural Local-Level Government Area</rdfs:label>
    </owl:NamedIndividual>
    


    <!-- http://purl.obolibrary.org/obo/GAZ_00118095 -->

    <owl:NamedIndividual rdf:about="http://purl.obolibrary.org/obo/GAZ_00118095">
        <obo:RO_0001025 rdf:resource="http://purl.obolibrary.org/obo/GAZ_00022400"/>
        <obo:IAO_0000115>A Local-Level Government Area of North Bougainville District.</obo:IAO_0000115>
        <oboInOwl:hasOBONamespace>GAZ</oboInOwl:hasOBONamespace>
        <oboInOwl:id>GAZ:00118095</oboInOwl:id>
        <rdfs:label>Atolls Rural Local-Level Government Area</rdfs:label>
    </owl:NamedIndividual>
    


    <!-- http://purl.obolibrary.org/obo/GAZ_00118096 -->

    <owl:NamedIndividual rdf:about="http://purl.obolibrary.org/obo/GAZ_00118096">
        <obo:RO_0001025 rdf:resource="http://purl.obolibrary.org/obo/GAZ_00022400"/>
        <obo:IAO_0000115>A Local-Level Government Area of North Bougainville District.</obo:IAO_0000115>
        <oboInOwl:hasOBONamespace>GAZ</oboInOwl:hasOBONamespace>
        <oboInOwl:id>GAZ:00118096</oboInOwl:id>
        <rdfs:label>Nissan Rural Local-Level Government Area</rdfs:label>
    </owl:NamedIndividual>
    


    <!-- http://purl.obolibrary.org/obo/GAZ_00118097 -->

    <owl:NamedIndividual rdf:about="http://purl.obolibrary.org/obo/GAZ_00118097">
        <obo:RO_0001025 rdf:resource="http://purl.obolibrary.org/obo/GAZ_00022400"/>
        <obo:IAO_0000115>A Local-Level Government Area of North Bougainville District.</obo:IAO_0000115>
        <oboInOwl:hasOBONamespace>GAZ</oboInOwl:hasOBONamespace>
        <oboInOwl:id>GAZ:00118097</oboInOwl:id>
        <rdfs:label>Tinputz Rural Local-Level Government Area</rdfs:label>
    </owl:NamedIndividual>
    


    <!-- http://purl.obolibrary.org/obo/GAZ_00118098 -->

    <owl:NamedIndividual rdf:about="http://purl.obolibrary.org/obo/GAZ_00118098">
        <obo:RO_0001025 rdf:resource="http://purl.obolibrary.org/obo/GAZ_00022400"/>
        <obo:IAO_0000115>A Local-Level Government Area of North Bougainville District.</obo:IAO_0000115>
        <oboInOwl:hasOBONamespace>GAZ</oboInOwl:hasOBONamespace>
        <oboInOwl:id>GAZ:00118098</oboInOwl:id>
        <rdfs:label>Kunua Rural Local-Level Government Area</rdfs:label>
    </owl:NamedIndividual>
    


    <!-- http://purl.obolibrary.org/obo/GAZ_00118099 -->

    <owl:NamedIndividual rdf:about="http://purl.obolibrary.org/obo/GAZ_00118099">
        <obo:RO_0001025 rdf:resource="http://purl.obolibrary.org/obo/GAZ_00022400"/>
        <obo:IAO_0000115>A Local-Level Government Area of North Bougainville District.</obo:IAO_0000115>
        <oboInOwl:hasOBONamespace>GAZ</oboInOwl:hasOBONamespace>
        <oboInOwl:id>GAZ:00118099</oboInOwl:id>
        <rdfs:label>Selau Suir Rural Local-Level Government Area</rdfs:label>
    </owl:NamedIndividual>
    


    <!-- http://purl.obolibrary.org/obo/GAZ_00118100 -->

    <owl:NamedIndividual rdf:about="http://purl.obolibrary.org/obo/GAZ_00118100">
        <obo:RO_0001025 rdf:resource="http://purl.obolibrary.org/obo/GAZ_00022400"/>
        <obo:IAO_0000115>A Local-Level Government Area of North Bougainville District.</obo:IAO_0000115>
        <oboInOwl:hasOBONamespace>GAZ</oboInOwl:hasOBONamespace>
        <oboInOwl:id>GAZ:00118100</oboInOwl:id>
        <rdfs:label>Buka Rural Local-Level Government Area</rdfs:label>
    </owl:NamedIndividual>
    


    <!-- http://purl.obolibrary.org/obo/GAZ_00118101 -->

    <owl:NamedIndividual rdf:about="http://purl.obolibrary.org/obo/GAZ_00118101">
        <obo:RO_0001025 rdf:resource="http://purl.obolibrary.org/obo/GAZ_00022396"/>
        <obo:IAO_0000115>A Local-Level Government Area of Kavieng District.</obo:IAO_0000115>
        <oboInOwl:hasOBONamespace>GAZ</oboInOwl:hasOBONamespace>
        <oboInOwl:id>GAZ:00118101</oboInOwl:id>
        <rdfs:label>Kavieng Urban Local-Level Government Area</rdfs:label>
    </owl:NamedIndividual>
    


    <!-- http://purl.obolibrary.org/obo/GAZ_00118102 -->

    <owl:NamedIndividual rdf:about="http://purl.obolibrary.org/obo/GAZ_00118102">
        <obo:RO_0001025 rdf:resource="http://purl.obolibrary.org/obo/GAZ_00022396"/>
        <obo:IAO_0000115>A Local-Level Government Area of Kavieng District. The LLG administers the island of New Hanover and a few surrounding islands.</obo:IAO_0000115>
        <oboInOwl:hasOBONamespace>GAZ</oboInOwl:hasOBONamespace>
        <oboInOwl:id>GAZ:00118102</oboInOwl:id>
        <rdfs:label>Lavongai Rural Local-Level Government Area</rdfs:label>
    </owl:NamedIndividual>
    


    <!-- http://purl.obolibrary.org/obo/GAZ_00118103 -->

    <owl:NamedIndividual rdf:about="http://purl.obolibrary.org/obo/GAZ_00118103">
        <obo:RO_0001025 rdf:resource="http://purl.obolibrary.org/obo/GAZ_00022396"/>
        <obo:IAO_0000115>A Local-Level Government Area of Kavieng District. The LLG administers the northern section of the island of New Ireland, as well as Dyaul Island and some Tigak islands in the strait between New Ireland and New Hanover.</obo:IAO_0000115>
        <oboInOwl:hasOBONamespace>GAZ</oboInOwl:hasOBONamespace>
        <oboInOwl:id>GAZ:00118103</oboInOwl:id>
        <rdfs:label>Tikana Rural Local-Level Government Area</rdfs:label>
    </owl:NamedIndividual>
    


    <!-- http://purl.obolibrary.org/obo/GAZ_00118104 -->

    <owl:NamedIndividual rdf:about="http://purl.obolibrary.org/obo/GAZ_00118104">
        <obo:RO_0001025 rdf:resource="http://purl.obolibrary.org/obo/GAZ_00022396"/>
        <obo:IAO_0000115>A Local-Level Government Area of Kavieng District. The LLG administers the St. Matthias Group of islands and is located in Kavieng District.</obo:IAO_0000115>
        <oboInOwl:hasOBONamespace>GAZ</oboInOwl:hasOBONamespace>
        <oboInOwl:id>GAZ:00118104</oboInOwl:id>
        <rdfs:label>Murat Rural Local-Level Government Area</rdfs:label>
    </owl:NamedIndividual>
    


    <!-- http://purl.obolibrary.org/obo/GAZ_00118105 -->

    <owl:NamedIndividual rdf:about="http://purl.obolibrary.org/obo/GAZ_00118105">
        <obo:RO_0001025 rdf:resource="http://purl.obolibrary.org/obo/GAZ_00022397"/>
        <obo:IAO_0000115>A Local-Level Government Area of Namatanai District. The LLG administers the southern peninsula of the island of New Ireland.</obo:IAO_0000115>
        <oboInOwl:hasOBONamespace>GAZ</oboInOwl:hasOBONamespace>
        <oboInOwl:id>GAZ:00118105</oboInOwl:id>
        <rdfs:label>Konoagil Rural Local-Level Government Area</rdfs:label>
    </owl:NamedIndividual>
    


    <!-- http://purl.obolibrary.org/obo/GAZ_00118106 -->

    <owl:NamedIndividual rdf:about="http://purl.obolibrary.org/obo/GAZ_00118106">
        <obo:RO_0001025 rdf:resource="http://purl.obolibrary.org/obo/GAZ_00022397"/>
        <obo:IAO_0000115>A Local-Level Government Area of Namatanai District. The LLG administers the Lihir Group of islands. The LLG is located in Namatanai District and contains the Lihir Gold Mine, which is the second largest gold deposit in the world.</obo:IAO_0000115>
        <oboInOwl:hasOBONamespace>GAZ</oboInOwl:hasOBONamespace>
        <oboInOwl:id>GAZ:00118106</oboInOwl:id>
        <rdfs:label>Nimamar Rural Local-Level Government Area</rdfs:label>
    </owl:NamedIndividual>
    


    <!-- http://purl.obolibrary.org/obo/GAZ_00118107 -->

    <owl:NamedIndividual rdf:about="http://purl.obolibrary.org/obo/GAZ_00118107">
        <obo:RO_0001025 rdf:resource="http://purl.obolibrary.org/obo/GAZ_00022397"/>
        <obo:IAO_0000115>A Local-Level Government Area of Namatanai District. The LLG administers the Tangga Group and the Feni Islands.</obo:IAO_0000115>
        <oboInOwl:hasOBONamespace>GAZ</oboInOwl:hasOBONamespace>
        <oboInOwl:id>GAZ:00118107</oboInOwl:id>
        <rdfs:label>Tanir Rural Local-Level Government Area</rdfs:label>
    </owl:NamedIndividual>
    


    <!-- http://purl.obolibrary.org/obo/GAZ_00118108 -->

    <owl:NamedIndividual rdf:about="http://purl.obolibrary.org/obo/GAZ_00118108">
        <obo:RO_0001025 rdf:resource="http://purl.obolibrary.org/obo/GAZ_00022397"/>
        <obo:IAO_0000115>A Local-Level Government Area of Namatanai District.</obo:IAO_0000115>
        <oboInOwl:hasOBONamespace>GAZ</oboInOwl:hasOBONamespace>
        <oboInOwl:id>GAZ:00118108</oboInOwl:id>
        <rdfs:label>Namatanai Rural Local-Level Government Area</rdfs:label>
    </owl:NamedIndividual>
    


    <!-- http://purl.obolibrary.org/obo/GAZ_00118109 -->

    <owl:NamedIndividual rdf:about="http://purl.obolibrary.org/obo/GAZ_00118109">
        <obo:RO_0001025 rdf:resource="http://purl.obolibrary.org/obo/GAZ_00022397"/>
        <obo:IAO_0000115>A Local-Level Government Area of Namatanai District. The LLG administers a central area of the island of New Ireland and the Tabar Group.</obo:IAO_0000115>
        <oboInOwl:hasOBONamespace>GAZ</oboInOwl:hasOBONamespace>
        <oboInOwl:id>GAZ:00118109</oboInOwl:id>
        <rdfs:label>Sentral Niu Ailan Rural Local-Level Government Area</rdfs:label>
    </owl:NamedIndividual>
    


    <!-- http://purl.obolibrary.org/obo/GAZ_00118110 -->

    <owl:NamedIndividual rdf:about="http://purl.obolibrary.org/obo/GAZ_00118110">
        <obo:RO_0001025 rdf:resource="http://purl.obolibrary.org/obo/GAZ_00022429"/>
        <obo:IAO_0000115>A Local-Level Government Area of Kandrian-Gloucester District.</obo:IAO_0000115>
        <oboInOwl:hasOBONamespace>GAZ</oboInOwl:hasOBONamespace>
        <oboInOwl:id>GAZ:00118110</oboInOwl:id>
        <rdfs:label>Gasmata Rural Local-Level Government Area</rdfs:label>
    </owl:NamedIndividual>
    


    <!-- http://purl.obolibrary.org/obo/GAZ_00118111 -->

    <owl:NamedIndividual rdf:about="http://purl.obolibrary.org/obo/GAZ_00118111">
        <obo:RO_0001025 rdf:resource="http://purl.obolibrary.org/obo/GAZ_00022429"/>
        <obo:IAO_0000115>A Local-Level Government Area of Kandrian-Gloucester District.</obo:IAO_0000115>
        <oboInOwl:hasOBONamespace>GAZ</oboInOwl:hasOBONamespace>
        <oboInOwl:id>GAZ:00118111</oboInOwl:id>
        <rdfs:label>Gloucester Rural Local-Level Government Area</rdfs:label>
    </owl:NamedIndividual>
    


    <!-- http://purl.obolibrary.org/obo/GAZ_00118112 -->

    <owl:NamedIndividual rdf:about="http://purl.obolibrary.org/obo/GAZ_00118112">
        <obo:RO_0001025 rdf:resource="http://purl.obolibrary.org/obo/GAZ_00022429"/>
        <obo:IAO_0000115>A Local-Level Government Area of Kandrian-Gloucester District.</obo:IAO_0000115>
        <oboInOwl:hasOBONamespace>GAZ</oboInOwl:hasOBONamespace>
        <oboInOwl:id>GAZ:00118112</oboInOwl:id>
        <rdfs:label>Kove-Kaliai Rural Local-Level Government Area</rdfs:label>
    </owl:NamedIndividual>
    


    <!-- http://purl.obolibrary.org/obo/GAZ_00118113 -->

    <owl:NamedIndividual rdf:about="http://purl.obolibrary.org/obo/GAZ_00118113">
        <obo:RO_0001025 rdf:resource="http://purl.obolibrary.org/obo/GAZ_00022429"/>
        <obo:IAO_0000115>A Local-Level Government Area of Kandrian-Gloucester District.</obo:IAO_0000115>
        <oboInOwl:hasOBONamespace>GAZ</oboInOwl:hasOBONamespace>
        <oboInOwl:id>GAZ:00118113</oboInOwl:id>
        <rdfs:label>Kandrian Coastal Rural Local-Level Government Area</rdfs:label>
    </owl:NamedIndividual>
    


    <!-- http://purl.obolibrary.org/obo/GAZ_00118114 -->

    <owl:NamedIndividual rdf:about="http://purl.obolibrary.org/obo/GAZ_00118114">
        <obo:RO_0001025 rdf:resource="http://purl.obolibrary.org/obo/GAZ_00022429"/>
        <obo:IAO_0000115>A Local-Level Government Area of Kandrian-Gloucester District.</obo:IAO_0000115>
        <oboInOwl:hasOBONamespace>GAZ</oboInOwl:hasOBONamespace>
        <oboInOwl:id>GAZ:00118114</oboInOwl:id>
        <rdfs:label>Kandrian Inland Rural Local-Level Government Area</rdfs:label>
    </owl:NamedIndividual>
    


    <!-- http://purl.obolibrary.org/obo/GAZ_00118115 -->

    <owl:NamedIndividual rdf:about="http://purl.obolibrary.org/obo/GAZ_00118115">
        <obo:RO_0001025 rdf:resource="http://purl.obolibrary.org/obo/GAZ_00022427"/>
        <obo:IAO_0000115>A Local-Level Government Area of Talasea District.</obo:IAO_0000115>
        <oboInOwl:hasOBONamespace>GAZ</oboInOwl:hasOBONamespace>
        <oboInOwl:id>GAZ:00118115</oboInOwl:id>
        <rdfs:label>Bali-Witu Rural Local-Level Government Area</rdfs:label>
    </owl:NamedIndividual>
    


    <!-- http://purl.obolibrary.org/obo/GAZ_00118116 -->

    <owl:NamedIndividual rdf:about="http://purl.obolibrary.org/obo/GAZ_00118116">
        <obo:RO_0001025 rdf:resource="http://purl.obolibrary.org/obo/GAZ_00022427"/>
        <obo:IAO_0000115>A Local-Level Government Area of Talasea District.</obo:IAO_0000115>
        <oboInOwl:hasOBONamespace>GAZ</oboInOwl:hasOBONamespace>
        <oboInOwl:id>GAZ:00118116</oboInOwl:id>
        <rdfs:label>Mosa Rural Local-Level Government Area</rdfs:label>
    </owl:NamedIndividual>
    


    <!-- http://purl.obolibrary.org/obo/GAZ_00118117 -->

    <owl:NamedIndividual rdf:about="http://purl.obolibrary.org/obo/GAZ_00118117">
        <obo:RO_0001025 rdf:resource="http://purl.obolibrary.org/obo/GAZ_00022427"/>
        <obo:IAO_0000115>A Local-Level Government Area of Talasea District.</obo:IAO_0000115>
        <oboInOwl:hasOBONamespace>GAZ</oboInOwl:hasOBONamespace>
        <oboInOwl:id>GAZ:00118117</oboInOwl:id>
        <rdfs:label>Talasea Rural Local-Level Government Area</rdfs:label>
    </owl:NamedIndividual>
    


    <!-- http://purl.obolibrary.org/obo/GAZ_00118118 -->

    <owl:NamedIndividual rdf:about="http://purl.obolibrary.org/obo/GAZ_00118118">
        <obo:RO_0001025 rdf:resource="http://purl.obolibrary.org/obo/GAZ_00022427"/>
        <obo:IAO_0000115>A Local-Level Government Area of Talasea District.</obo:IAO_0000115>
        <oboInOwl:hasOBONamespace>GAZ</oboInOwl:hasOBONamespace>
        <oboInOwl:id>GAZ:00118118</oboInOwl:id>
        <rdfs:label>Hoskins Rural Local-Level Government Area</rdfs:label>
    </owl:NamedIndividual>
    


    <!-- http://purl.obolibrary.org/obo/GAZ_00118119 -->

    <owl:NamedIndividual rdf:about="http://purl.obolibrary.org/obo/GAZ_00118119">
        <obo:RO_0001025 rdf:resource="http://purl.obolibrary.org/obo/GAZ_00022427"/>
        <obo:IAO_0000115>A Local-Level Government Area of Talasea District.</obo:IAO_0000115>
        <oboInOwl:hasOBONamespace>GAZ</oboInOwl:hasOBONamespace>
        <oboInOwl:id>GAZ:00118119</oboInOwl:id>
        <rdfs:label>Kimbe Urban Local-Level Government Area</rdfs:label>
    </owl:NamedIndividual>
    


    <!-- http://purl.obolibrary.org/obo/GAZ_00118120 -->

    <owl:NamedIndividual rdf:about="http://purl.obolibrary.org/obo/GAZ_00118120">
        <obo:RO_0001025 rdf:resource="http://purl.obolibrary.org/obo/GAZ_00022427"/>
        <obo:IAO_0000115>A Local-Level Government Area of Talasea District.</obo:IAO_0000115>
        <oboInOwl:hasOBONamespace>GAZ</oboInOwl:hasOBONamespace>
        <oboInOwl:id>GAZ:00118120</oboInOwl:id>
        <rdfs:label>Bialla Rural Local-Level Government Area</rdfs:label>
    </owl:NamedIndividual>
    


    <!-- http://purl.obolibrary.org/obo/GAZ_00118121 -->

    <owl:NamedIndividual rdf:about="http://purl.obolibrary.org/obo/GAZ_00118121">
        <obo:RO_0001025 rdf:resource="http://purl.obolibrary.org/obo/GAZ_00022413"/>
        <oboInOwl:hasOBONamespace>GAZ</oboInOwl:hasOBONamespace>
        <oboInOwl:id>GAZ:00118121</oboInOwl:id>
        <rdfs:label>Chauve Rural Local-Level Government Area</rdfs:label>
    </owl:NamedIndividual>
    


    <!-- http://purl.obolibrary.org/obo/GAZ_00118122 -->

    <owl:NamedIndividual rdf:about="http://purl.obolibrary.org/obo/GAZ_00118122">
        <obo:RO_0001025 rdf:resource="http://purl.obolibrary.org/obo/GAZ_00022413"/>
        <oboInOwl:hasOBONamespace>GAZ</oboInOwl:hasOBONamespace>
        <oboInOwl:id>GAZ:00118122</oboInOwl:id>
        <rdfs:label>Elimbari Rural Local-Level Government Area</rdfs:label>
    </owl:NamedIndividual>
    


    <!-- http://purl.obolibrary.org/obo/GAZ_00118123 -->

    <owl:NamedIndividual rdf:about="http://purl.obolibrary.org/obo/GAZ_00118123">
        <obo:RO_0001025 rdf:resource="http://purl.obolibrary.org/obo/GAZ_00022413"/>
        <oboInOwl:hasOBONamespace>GAZ</oboInOwl:hasOBONamespace>
        <oboInOwl:id>GAZ:00118123</oboInOwl:id>
        <rdfs:label>Siane Rural Local-Level Government Area</rdfs:label>
    </owl:NamedIndividual>
    


    <!-- http://purl.obolibrary.org/obo/GAZ_00118124 -->

    <owl:NamedIndividual rdf:about="http://purl.obolibrary.org/obo/GAZ_00118124">
        <obo:RO_0001025 rdf:resource="http://purl.obolibrary.org/obo/GAZ_00022416"/>
        <oboInOwl:hasOBONamespace>GAZ</oboInOwl:hasOBONamespace>
        <oboInOwl:id>GAZ:00118124</oboInOwl:id>
        <rdfs:label>Gumine Rural Local-Level Government Area</rdfs:label>
    </owl:NamedIndividual>
    


    <!-- http://purl.obolibrary.org/obo/GAZ_00118125 -->

    <owl:NamedIndividual rdf:about="http://purl.obolibrary.org/obo/GAZ_00118125">
        <obo:RO_0001025 rdf:resource="http://purl.obolibrary.org/obo/GAZ_00022416"/>
        <oboInOwl:hasOBONamespace>GAZ</oboInOwl:hasOBONamespace>
        <oboInOwl:id>GAZ:00118125</oboInOwl:id>
        <rdfs:label>Bomai-Kumai Rural Local-Level Government Area</rdfs:label>
    </owl:NamedIndividual>
    


    <!-- http://purl.obolibrary.org/obo/GAZ_00118126 -->

    <owl:NamedIndividual rdf:about="http://purl.obolibrary.org/obo/GAZ_00118126">
        <obo:RO_0001025 rdf:resource="http://purl.obolibrary.org/obo/GAZ_00022416"/>
        <oboInOwl:hasOBONamespace>GAZ</oboInOwl:hasOBONamespace>
        <oboInOwl:id>GAZ:00118126</oboInOwl:id>
        <rdfs:label>Mount Digine Rural Local-Level Government Area</rdfs:label>
    </owl:NamedIndividual>
    


    <!-- http://purl.obolibrary.org/obo/GAZ_00118127 -->

    <owl:NamedIndividual rdf:about="http://purl.obolibrary.org/obo/GAZ_00118127">
        <obo:RO_0001025 rdf:resource="http://purl.obolibrary.org/obo/GAZ_00022412"/>
        <oboInOwl:hasOBONamespace>GAZ</oboInOwl:hasOBONamespace>
        <oboInOwl:id>GAZ:00118127</oboInOwl:id>
        <rdfs:label>Karimui Rural Local-Level Government Area</rdfs:label>
    </owl:NamedIndividual>
    


    <!-- http://purl.obolibrary.org/obo/GAZ_00118128 -->

    <owl:NamedIndividual rdf:about="http://purl.obolibrary.org/obo/GAZ_00118128">
        <obo:RO_0001025 rdf:resource="http://purl.obolibrary.org/obo/GAZ_00022412"/>
        <oboInOwl:hasOBONamespace>GAZ</oboInOwl:hasOBONamespace>
        <oboInOwl:id>GAZ:00118128</oboInOwl:id>
        <rdfs:label>Nomane Rural Local-Level Government Area</rdfs:label>
    </owl:NamedIndividual>
    


    <!-- http://purl.obolibrary.org/obo/GAZ_00118129 -->

    <owl:NamedIndividual rdf:about="http://purl.obolibrary.org/obo/GAZ_00118129">
        <obo:RO_0001025 rdf:resource="http://purl.obolibrary.org/obo/GAZ_00022412"/>
        <oboInOwl:hasOBONamespace>GAZ</oboInOwl:hasOBONamespace>
        <oboInOwl:id>GAZ:00118129</oboInOwl:id>
        <rdfs:label>Salt Rural Local-Level Government Area</rdfs:label>
    </owl:NamedIndividual>
    


    <!-- http://purl.obolibrary.org/obo/GAZ_00118130 -->

    <owl:NamedIndividual rdf:about="http://purl.obolibrary.org/obo/GAZ_00118130">
        <obo:RO_0001025 rdf:resource="http://purl.obolibrary.org/obo/GAZ_00022414"/>
        <oboInOwl:hasOBONamespace>GAZ</oboInOwl:hasOBONamespace>
        <oboInOwl:id>GAZ:00118130</oboInOwl:id>
        <rdfs:label>Gena-Waugla Rural Local-Level Government Area</rdfs:label>
    </owl:NamedIndividual>
    


    <!-- http://purl.obolibrary.org/obo/GAZ_00118131 -->

    <owl:NamedIndividual rdf:about="http://purl.obolibrary.org/obo/GAZ_00118131">
        <obo:RO_0001025 rdf:resource="http://purl.obolibrary.org/obo/GAZ_00022414"/>
        <oboInOwl:hasOBONamespace>GAZ</oboInOwl:hasOBONamespace>
        <oboInOwl:id>GAZ:00118131</oboInOwl:id>
        <rdfs:label>Kerowagi Rural Local-Level Government Area</rdfs:label>
    </owl:NamedIndividual>
    


    <!-- http://purl.obolibrary.org/obo/GAZ_00118132 -->

    <owl:NamedIndividual rdf:about="http://purl.obolibrary.org/obo/GAZ_00118132">
        <obo:RO_0001025 rdf:resource="http://purl.obolibrary.org/obo/GAZ_00022414"/>
        <oboInOwl:hasOBONamespace>GAZ</oboInOwl:hasOBONamespace>
        <oboInOwl:id>GAZ:00118132</oboInOwl:id>
        <rdfs:label>Kup Rural Local-Level Government Area</rdfs:label>
    </owl:NamedIndividual>
    


    <!-- http://purl.obolibrary.org/obo/GAZ_00118133 -->

    <owl:NamedIndividual rdf:about="http://purl.obolibrary.org/obo/GAZ_00118133">
        <obo:RO_0001025 rdf:resource="http://purl.obolibrary.org/obo/GAZ_00022415"/>
        <oboInOwl:hasOBONamespace>GAZ</oboInOwl:hasOBONamespace>
        <oboInOwl:id>GAZ:00118133</oboInOwl:id>
        <rdfs:label>Kundiawa Urban Local-Level Government Area</rdfs:label>
    </owl:NamedIndividual>
    


    <!-- http://purl.obolibrary.org/obo/GAZ_00118134 -->

    <owl:NamedIndividual rdf:about="http://purl.obolibrary.org/obo/GAZ_00118134">
        <obo:RO_0001025 rdf:resource="http://purl.obolibrary.org/obo/GAZ_00022415"/>
        <oboInOwl:hasOBONamespace>GAZ</oboInOwl:hasOBONamespace>
        <oboInOwl:id>GAZ:00118134</oboInOwl:id>
        <rdfs:label>Mount Wilhelm Rural Local-Level Government Area</rdfs:label>
    </owl:NamedIndividual>
    


    <!-- http://purl.obolibrary.org/obo/GAZ_00118135 -->

    <owl:NamedIndividual rdf:about="http://purl.obolibrary.org/obo/GAZ_00118135">
        <obo:RO_0001025 rdf:resource="http://purl.obolibrary.org/obo/GAZ_00022415"/>
        <oboInOwl:hasOBONamespace>GAZ</oboInOwl:hasOBONamespace>
        <oboInOwl:id>GAZ:00118135</oboInOwl:id>
        <rdfs:label>Waiye Rural Local-Level Government Area</rdfs:label>
    </owl:NamedIndividual>
    


    <!-- http://purl.obolibrary.org/obo/GAZ_00118136 -->

    <owl:NamedIndividual rdf:about="http://purl.obolibrary.org/obo/GAZ_00118136">
        <obo:RO_0001025 rdf:resource="http://purl.obolibrary.org/obo/GAZ_00022415"/>
        <oboInOwl:hasOBONamespace>GAZ</oboInOwl:hasOBONamespace>
        <oboInOwl:id>GAZ:00118136</oboInOwl:id>
        <rdfs:label>Niglkande Rural Local-Level Government Area</rdfs:label>
    </owl:NamedIndividual>
    


    <!-- http://purl.obolibrary.org/obo/GAZ_00118137 -->

    <owl:NamedIndividual rdf:about="http://purl.obolibrary.org/obo/GAZ_00118137">
        <obo:RO_0001025 rdf:resource="http://purl.obolibrary.org/obo/GAZ_00022411"/>
        <oboInOwl:hasOBONamespace>GAZ</oboInOwl:hasOBONamespace>
        <oboInOwl:id>GAZ:00118137</oboInOwl:id>
        <rdfs:label>Sinasina Rural Local-Level Government Area</rdfs:label>
    </owl:NamedIndividual>
    


    <!-- http://purl.obolibrary.org/obo/GAZ_00118138 -->

    <owl:NamedIndividual rdf:about="http://purl.obolibrary.org/obo/GAZ_00118138">
        <obo:RO_0001025 rdf:resource="http://purl.obolibrary.org/obo/GAZ_00022411"/>
        <oboInOwl:hasOBONamespace>GAZ</oboInOwl:hasOBONamespace>
        <oboInOwl:id>GAZ:00118138</oboInOwl:id>
        <rdfs:label>Suwai Rural Local-Level Government Area</rdfs:label>
    </owl:NamedIndividual>
    


    <!-- http://purl.obolibrary.org/obo/GAZ_00118139 -->

    <owl:NamedIndividual rdf:about="http://purl.obolibrary.org/obo/GAZ_00118139">
        <obo:RO_0001025 rdf:resource="http://purl.obolibrary.org/obo/GAZ_00022411"/>
        <oboInOwl:hasOBONamespace>GAZ</oboInOwl:hasOBONamespace>
        <oboInOwl:id>GAZ:00118139</oboInOwl:id>
        <rdfs:label>Yonggomugl Rural Local-Level Government Area</rdfs:label>
    </owl:NamedIndividual>
    


    <!-- http://purl.obolibrary.org/obo/GAZ_00118140 -->

    <owl:NamedIndividual rdf:about="http://purl.obolibrary.org/obo/GAZ_00118140">
        <obo:RO_0001025 rdf:resource="http://purl.obolibrary.org/obo/GAZ_00022343"/>
        <oboInOwl:hasOBONamespace>GAZ</oboInOwl:hasOBONamespace>
        <oboInOwl:id>GAZ:00118140</oboInOwl:id>
        <rdfs:label>Asaro-Watabung Rural Local-Level Government Area</rdfs:label>
    </owl:NamedIndividual>
    


    <!-- http://purl.obolibrary.org/obo/GAZ_00118141 -->

    <owl:NamedIndividual rdf:about="http://purl.obolibrary.org/obo/GAZ_00118141">
        <obo:RO_0001025 rdf:resource="http://purl.obolibrary.org/obo/GAZ_00022344"/>
        <oboInOwl:hasOBONamespace>GAZ</oboInOwl:hasOBONamespace>
        <oboInOwl:id>GAZ:00118141</oboInOwl:id>
        <rdfs:label>Henganofi Rural Local-Level Government Area</rdfs:label>
    </owl:NamedIndividual>
    


    <!-- http://purl.obolibrary.org/obo/GAZ_00118142 -->

    <owl:NamedIndividual rdf:about="http://purl.obolibrary.org/obo/GAZ_00118142">
        <obo:RO_0001025 rdf:resource="http://purl.obolibrary.org/obo/GAZ_00022337"/>
        <oboInOwl:hasOBONamespace>GAZ</oboInOwl:hasOBONamespace>
        <oboInOwl:id>GAZ:00118142</oboInOwl:id>
        <rdfs:label>Kainantu Rural Local-Level Government Area</rdfs:label>
    </owl:NamedIndividual>
    


    <!-- http://purl.obolibrary.org/obo/GAZ_00118143 -->

    <owl:NamedIndividual rdf:about="http://purl.obolibrary.org/obo/GAZ_00118143">
        <obo:RO_0001025 rdf:resource="http://purl.obolibrary.org/obo/GAZ_00022337"/>
        <oboInOwl:hasOBONamespace>GAZ</oboInOwl:hasOBONamespace>
        <oboInOwl:id>GAZ:00118143</oboInOwl:id>
        <rdfs:label>Kainantu Urban Local-Level Government Area</rdfs:label>
    </owl:NamedIndividual>
    


    <!-- http://purl.obolibrary.org/obo/GAZ_00118144 -->

    <owl:NamedIndividual rdf:about="http://purl.obolibrary.org/obo/GAZ_00118144">
        <obo:RO_0001025 rdf:resource="http://purl.obolibrary.org/obo/GAZ_00022342"/>
        <oboInOwl:hasOBONamespace>GAZ</oboInOwl:hasOBONamespace>
        <oboInOwl:id>GAZ:00118144</oboInOwl:id>
        <rdfs:label>Lufa Rural Local-Level Government Area</rdfs:label>
    </owl:NamedIndividual>
    


    <!-- http://purl.obolibrary.org/obo/GAZ_00118145 -->

    <owl:NamedIndividual rdf:about="http://purl.obolibrary.org/obo/GAZ_00118145">
        <obo:RO_0001025 rdf:resource="http://purl.obolibrary.org/obo/GAZ_00022338"/>
        <oboInOwl:hasOBONamespace>GAZ</oboInOwl:hasOBONamespace>
        <oboInOwl:id>GAZ:00118145</oboInOwl:id>
        <rdfs:label>Lamari Rural Local-Level Government Area</rdfs:label>
    </owl:NamedIndividual>
    


    <!-- http://purl.obolibrary.org/obo/GAZ_00118146 -->

    <owl:NamedIndividual rdf:about="http://purl.obolibrary.org/obo/GAZ_00118146">
        <obo:RO_0001025 rdf:resource="http://purl.obolibrary.org/obo/GAZ_00022338"/>
        <oboInOwl:hasOBONamespace>GAZ</oboInOwl:hasOBONamespace>
        <oboInOwl:id>GAZ:00118146</oboInOwl:id>
        <rdfs:label>Yelia Rural Local-Level Government Area</rdfs:label>
    </owl:NamedIndividual>
    


    <!-- http://purl.obolibrary.org/obo/GAZ_00118147 -->

    <owl:NamedIndividual rdf:about="http://purl.obolibrary.org/obo/GAZ_00118147">
        <obo:RO_0001025 rdf:resource="http://purl.obolibrary.org/obo/GAZ_00022340"/>
        <oboInOwl:hasOBONamespace>GAZ</oboInOwl:hasOBONamespace>
        <oboInOwl:id>GAZ:00118147</oboInOwl:id>
        <rdfs:label>Okapa Rural Local-Level Government Area</rdfs:label>
    </owl:NamedIndividual>
    


    <!-- http://purl.obolibrary.org/obo/GAZ_00118148 -->

    <owl:NamedIndividual rdf:about="http://purl.obolibrary.org/obo/GAZ_00118148">
        <obo:RO_0001025 rdf:resource="http://purl.obolibrary.org/obo/GAZ_00022339"/>
        <oboInOwl:hasOBONamespace>GAZ</oboInOwl:hasOBONamespace>
        <oboInOwl:id>GAZ:00118148</oboInOwl:id>
        <rdfs:label>Unggai-Benna Rural Local-Level Government Area</rdfs:label>
    </owl:NamedIndividual>
    


    <!-- http://purl.obolibrary.org/obo/GAZ_00118149 -->

    <owl:NamedIndividual rdf:about="http://purl.obolibrary.org/obo/GAZ_00118149">
        <obo:RO_0001025 rdf:resource="http://purl.obolibrary.org/obo/GAZ_00022357"/>
        <obo:IAO_0000115>A Local-Level Government Area of Kandep District.</obo:IAO_0000115>
        <oboInOwl:hasOBONamespace>GAZ</oboInOwl:hasOBONamespace>
        <oboInOwl:id>GAZ:00118149</oboInOwl:id>
        <rdfs:label>Kandep Rural Local-Level Government Area</rdfs:label>
    </owl:NamedIndividual>
    


    <!-- http://purl.obolibrary.org/obo/GAZ_00118150 -->

    <owl:NamedIndividual rdf:about="http://purl.obolibrary.org/obo/GAZ_00118150">
        <obo:RO_0001025 rdf:resource="http://purl.obolibrary.org/obo/GAZ_00022357"/>
        <obo:IAO_0000115>A Local-Level Government Area of Kandep District.</obo:IAO_0000115>
        <oboInOwl:hasOBONamespace>GAZ</oboInOwl:hasOBONamespace>
        <oboInOwl:id>GAZ:00118150</oboInOwl:id>
        <rdfs:label>Wage Rural Local-Level Government Area</rdfs:label>
    </owl:NamedIndividual>
    


    <!-- http://purl.obolibrary.org/obo/GAZ_00118151 -->

    <owl:NamedIndividual rdf:about="http://purl.obolibrary.org/obo/GAZ_00118151">
        <obo:RO_0001025 rdf:resource="http://purl.obolibrary.org/obo/GAZ_00022356"/>
        <obo:IAO_0000115>A Local-Level Government Area of Kompian District.</obo:IAO_0000115>
        <oboInOwl:hasOBONamespace>GAZ</oboInOwl:hasOBONamespace>
        <oboInOwl:id>GAZ:00118151</oboInOwl:id>
        <rdfs:label>Ambum Rural Local-Level Government Area</rdfs:label>
    </owl:NamedIndividual>
    


    <!-- http://purl.obolibrary.org/obo/GAZ_00118152 -->

    <owl:NamedIndividual rdf:about="http://purl.obolibrary.org/obo/GAZ_00118152">
        <obo:RO_0001025 rdf:resource="http://purl.obolibrary.org/obo/GAZ_00022356"/>
        <obo:IAO_0000115>A Local-Level Government Area of Kompian District.</obo:IAO_0000115>
        <oboInOwl:hasOBONamespace>GAZ</oboInOwl:hasOBONamespace>
        <oboInOwl:id>GAZ:00118152</oboInOwl:id>
        <rdfs:label>Kompiam Rural Local-Level Government Area</rdfs:label>
    </owl:NamedIndividual>
    


    <!-- http://purl.obolibrary.org/obo/GAZ_00118153 -->

    <owl:NamedIndividual rdf:about="http://purl.obolibrary.org/obo/GAZ_00118153">
        <obo:RO_0001025 rdf:resource="http://purl.obolibrary.org/obo/GAZ_00022356"/>
        <obo:IAO_0000115>A Local-Level Government Area of Kompian District.</obo:IAO_0000115>
        <oboInOwl:hasOBONamespace>GAZ</oboInOwl:hasOBONamespace>
        <oboInOwl:id>GAZ:00118153</oboInOwl:id>
        <rdfs:label>Wapi (Uangis) Rural Local-Level Government Area</rdfs:label>
    </owl:NamedIndividual>
    


    <!-- http://purl.obolibrary.org/obo/GAZ_00118154 -->

    <owl:NamedIndividual rdf:about="http://purl.obolibrary.org/obo/GAZ_00118154">
        <obo:RO_0001025 rdf:resource="http://purl.obolibrary.org/obo/GAZ_00022358"/>
        <obo:IAO_0000115>A Local-Level Government Area of Lagaip-Porgera District.</obo:IAO_0000115>
        <oboInOwl:hasOBONamespace>GAZ</oboInOwl:hasOBONamespace>
        <oboInOwl:id>GAZ:00118154</oboInOwl:id>
        <rdfs:label>Lagaip Rural Local-Level Government Area</rdfs:label>
    </owl:NamedIndividual>
    


    <!-- http://purl.obolibrary.org/obo/GAZ_00118155 -->

    <owl:NamedIndividual rdf:about="http://purl.obolibrary.org/obo/GAZ_00118155">
        <obo:RO_0001025 rdf:resource="http://purl.obolibrary.org/obo/GAZ_00022358"/>
        <obo:IAO_0000115>A Local-Level Government Area of Lagaip-Porgera District.</obo:IAO_0000115>
        <oboInOwl:hasOBONamespace>GAZ</oboInOwl:hasOBONamespace>
        <oboInOwl:id>GAZ:00118155</oboInOwl:id>
        <rdfs:label>Maip-Mulitaka Rural Local-Level Government Area</rdfs:label>
    </owl:NamedIndividual>
    


    <!-- http://purl.obolibrary.org/obo/GAZ_00118156 -->

    <owl:NamedIndividual rdf:about="http://purl.obolibrary.org/obo/GAZ_00118156">
        <obo:RO_0001025 rdf:resource="http://purl.obolibrary.org/obo/GAZ_00022358"/>
        <obo:IAO_0000115>A Local-Level Government Area of Lagaip-Porgera District.</obo:IAO_0000115>
        <oboInOwl:hasOBONamespace>GAZ</oboInOwl:hasOBONamespace>
        <oboInOwl:id>GAZ:00118156</oboInOwl:id>
        <rdfs:label>Pogera Rural Local-Level Government Area</rdfs:label>
    </owl:NamedIndividual>
    


    <!-- http://purl.obolibrary.org/obo/GAZ_00118157 -->

    <owl:NamedIndividual rdf:about="http://purl.obolibrary.org/obo/GAZ_00118157">
        <obo:RO_0001025 rdf:resource="http://purl.obolibrary.org/obo/GAZ_00022358"/>
        <obo:IAO_0000115>A Local-Level Government Area of Lagaip-Porgera District.</obo:IAO_0000115>
        <oboInOwl:hasOBONamespace>GAZ</oboInOwl:hasOBONamespace>
        <oboInOwl:id>GAZ:00118157</oboInOwl:id>
        <rdfs:label>Paiela-Hewa Rural Local-Level Government Area</rdfs:label>
    </owl:NamedIndividual>
    


    <!-- http://purl.obolibrary.org/obo/GAZ_00118158 -->

    <owl:NamedIndividual rdf:about="http://purl.obolibrary.org/obo/GAZ_00118158">
        <obo:RO_0001025 rdf:resource="http://purl.obolibrary.org/obo/GAZ_00022357"/>
        <obo:IAO_0000115>A Local-Level Government Area of Kandep District.</obo:IAO_0000115>
        <oboInOwl:hasOBONamespace>GAZ</oboInOwl:hasOBONamespace>
        <oboInOwl:id>GAZ:00118158</oboInOwl:id>
        <rdfs:label>Tsak Rural Local-Level Government Area</rdfs:label>
    </owl:NamedIndividual>
    


    <!-- http://purl.obolibrary.org/obo/GAZ_00118159 -->

    <owl:NamedIndividual rdf:about="http://purl.obolibrary.org/obo/GAZ_00118159">
        <obo:RO_0001025 rdf:resource="http://purl.obolibrary.org/obo/GAZ_00022357"/>
        <obo:IAO_0000115>A Local-Level Government Area of Kandep District.</obo:IAO_0000115>
        <oboInOwl:hasOBONamespace>GAZ</oboInOwl:hasOBONamespace>
        <oboInOwl:id>GAZ:00118159</oboInOwl:id>
        <rdfs:label>Wapenamanda Rural Local-Level Government Area</rdfs:label>
    </owl:NamedIndividual>
    


    <!-- http://purl.obolibrary.org/obo/GAZ_00118160 -->

    <owl:NamedIndividual rdf:about="http://purl.obolibrary.org/obo/GAZ_00118160">
        <obo:RO_0001025 rdf:resource="http://purl.obolibrary.org/obo/GAZ_00022359"/>
        <obo:IAO_0000115>A Local-Level Government Area of Wabag District.</obo:IAO_0000115>
        <oboInOwl:hasOBONamespace>GAZ</oboInOwl:hasOBONamespace>
        <oboInOwl:id>GAZ:00118160</oboInOwl:id>
        <rdfs:label>Maramuni Rural Local-Level Government Area</rdfs:label>
    </owl:NamedIndividual>
    


    <!-- http://purl.obolibrary.org/obo/GAZ_00118161 -->

    <owl:NamedIndividual rdf:about="http://purl.obolibrary.org/obo/GAZ_00118161">
        <obo:RO_0001025 rdf:resource="http://purl.obolibrary.org/obo/GAZ_00022359"/>
        <obo:IAO_0000115>A Local-Level Government Area of Wabag District.</obo:IAO_0000115>
        <oboInOwl:hasOBONamespace>GAZ</oboInOwl:hasOBONamespace>
        <oboInOwl:id>GAZ:00118161</oboInOwl:id>
        <rdfs:label>Wabag Rural Local-Level Government Area</rdfs:label>
    </owl:NamedIndividual>
    


    <!-- http://purl.obolibrary.org/obo/GAZ_00118162 -->

    <owl:NamedIndividual rdf:about="http://purl.obolibrary.org/obo/GAZ_00118162">
        <obo:RO_0001025 rdf:resource="http://purl.obolibrary.org/obo/GAZ_00022359"/>
        <obo:IAO_0000115>A Local-Level Government Area of Wabag District.</obo:IAO_0000115>
        <oboInOwl:hasOBONamespace>GAZ</oboInOwl:hasOBONamespace>
        <oboInOwl:id>GAZ:00118162</oboInOwl:id>
        <rdfs:label>Wabag Urban Local-Level Government Area</rdfs:label>
    </owl:NamedIndividual>
    


    <!-- http://purl.obolibrary.org/obo/GAZ_00118163 -->

    <owl:NamedIndividual rdf:about="http://purl.obolibrary.org/obo/GAZ_00118163">
        <obo:RO_0001025 rdf:resource="http://purl.obolibrary.org/obo/GAZ_00022437"/>
        <obo:IAO_0000115>A Local-Level Government of Ialibu-Pangia District.</obo:IAO_0000115>
        <oboInOwl:hasOBONamespace>GAZ</oboInOwl:hasOBONamespace>
        <oboInOwl:id>GAZ:00118163</oboInOwl:id>
        <rdfs:label>Ialibu Urban Local-Level Government Area</rdfs:label>
    </owl:NamedIndividual>
    


    <!-- http://purl.obolibrary.org/obo/GAZ_00118164 -->

    <owl:NamedIndividual rdf:about="http://purl.obolibrary.org/obo/GAZ_00118164">
        <obo:RO_0001025 rdf:resource="http://purl.obolibrary.org/obo/GAZ_00022437"/>
        <obo:IAO_0000115>A Local-Level Government of Ialibu-Pangia District.</obo:IAO_0000115>
        <oboInOwl:hasOBONamespace>GAZ</oboInOwl:hasOBONamespace>
        <oboInOwl:id>GAZ:00118164</oboInOwl:id>
        <rdfs:label>East Pangia Rural Local-Level Government Area</rdfs:label>
    </owl:NamedIndividual>
    


    <!-- http://purl.obolibrary.org/obo/GAZ_00118165 -->

    <owl:NamedIndividual rdf:about="http://purl.obolibrary.org/obo/GAZ_00118165">
        <obo:RO_0001025 rdf:resource="http://purl.obolibrary.org/obo/GAZ_00022437"/>
        <obo:IAO_0000115>A Local-Level Government of Ialibu-Pangia District.</obo:IAO_0000115>
        <oboInOwl:hasOBONamespace>GAZ</oboInOwl:hasOBONamespace>
        <oboInOwl:id>GAZ:00118165</oboInOwl:id>
        <rdfs:label>Wiru Rural Local-Level Government Area</rdfs:label>
    </owl:NamedIndividual>
    


    <!-- http://purl.obolibrary.org/obo/GAZ_00118166 -->

    <owl:NamedIndividual rdf:about="http://purl.obolibrary.org/obo/GAZ_00118166">
        <obo:RO_0001025 rdf:resource="http://purl.obolibrary.org/obo/GAZ_00022437"/>
        <obo:IAO_0000115>A Local-Level Government of Ialibu-Pangia District.</obo:IAO_0000115>
        <oboInOwl:hasOBONamespace>GAZ</oboInOwl:hasOBONamespace>
        <oboInOwl:id>GAZ:00118166</oboInOwl:id>
        <rdfs:label>Kewabi Rural Local-Level Government Area</rdfs:label>
    </owl:NamedIndividual>
    


    <!-- http://purl.obolibrary.org/obo/GAZ_00118167 -->

    <owl:NamedIndividual rdf:about="http://purl.obolibrary.org/obo/GAZ_00118167">
        <obo:RO_0001025 rdf:resource="http://purl.obolibrary.org/obo/GAZ_00022436"/>
        <obo:IAO_0000115>A Local-Level Government of Imbonggu District.</obo:IAO_0000115>
        <oboInOwl:hasOBONamespace>GAZ</oboInOwl:hasOBONamespace>
        <oboInOwl:id>GAZ:00118167</oboInOwl:id>
        <rdfs:label>Ialibu Basin Rural Local-Level Government Area</rdfs:label>
    </owl:NamedIndividual>
    


    <!-- http://purl.obolibrary.org/obo/GAZ_00118168 -->

    <owl:NamedIndividual rdf:about="http://purl.obolibrary.org/obo/GAZ_00118168">
        <obo:RO_0001025 rdf:resource="http://purl.obolibrary.org/obo/GAZ_00022436"/>
        <obo:IAO_0000115>A Local-Level Government of Imbonggu District.</obo:IAO_0000115>
        <oboInOwl:hasOBONamespace>GAZ</oboInOwl:hasOBONamespace>
        <oboInOwl:id>GAZ:00118168</oboInOwl:id>
        <rdfs:label>Imbongu Rural Local-Level Government Area</rdfs:label>
    </owl:NamedIndividual>
    


    <!-- http://purl.obolibrary.org/obo/GAZ_00118169 -->

    <owl:NamedIndividual rdf:about="http://purl.obolibrary.org/obo/GAZ_00118169">
        <obo:RO_0001025 rdf:resource="http://purl.obolibrary.org/obo/GAZ_00022436"/>
        <obo:IAO_0000115>A Local-Level Government of Imbonggu District.</obo:IAO_0000115>
        <oboInOwl:hasOBONamespace>GAZ</oboInOwl:hasOBONamespace>
        <oboInOwl:id>GAZ:00118169</oboInOwl:id>
        <rdfs:label>Lower Mendi Rural Local-Level Government Area</rdfs:label>
    </owl:NamedIndividual>
    


    <!-- http://purl.obolibrary.org/obo/GAZ_00118170 -->

    <owl:NamedIndividual rdf:about="http://purl.obolibrary.org/obo/GAZ_00118170">
        <obo:RO_0001025 rdf:resource="http://purl.obolibrary.org/obo/GAZ_00022438"/>
        <obo:IAO_0000115>A Local-Level Government of Kagua-Erave District.</obo:IAO_0000115>
        <oboInOwl:hasOBONamespace>GAZ</oboInOwl:hasOBONamespace>
        <oboInOwl:id>GAZ:00118170</oboInOwl:id>
        <rdfs:label>Erave Rural Local-Level Government Area</rdfs:label>
    </owl:NamedIndividual>
    


    <!-- http://purl.obolibrary.org/obo/GAZ_00118171 -->

    <owl:NamedIndividual rdf:about="http://purl.obolibrary.org/obo/GAZ_00118171">
        <obo:RO_0001025 rdf:resource="http://purl.obolibrary.org/obo/GAZ_00022438"/>
        <obo:IAO_0000115>A Local-Level Government of Kagua-Erave District.</obo:IAO_0000115>
        <oboInOwl:hasOBONamespace>GAZ</oboInOwl:hasOBONamespace>
        <oboInOwl:id>GAZ:00118171</oboInOwl:id>
        <rdfs:label>Kagua Rural Local-Level Government Area</rdfs:label>
    </owl:NamedIndividual>
    


    <!-- http://purl.obolibrary.org/obo/GAZ_00118172 -->

    <owl:NamedIndividual rdf:about="http://purl.obolibrary.org/obo/GAZ_00118172">
        <obo:RO_0001025 rdf:resource="http://purl.obolibrary.org/obo/GAZ_00022438"/>
        <obo:IAO_0000115>A Local-Level Government of Kagua-Erave District.</obo:IAO_0000115>
        <oboInOwl:hasOBONamespace>GAZ</oboInOwl:hasOBONamespace>
        <oboInOwl:id>GAZ:00118172</oboInOwl:id>
        <rdfs:label>Kuare Rural Local-Level Government Area</rdfs:label>
    </owl:NamedIndividual>
    


    <!-- http://purl.obolibrary.org/obo/GAZ_00118173 -->

    <owl:NamedIndividual rdf:about="http://purl.obolibrary.org/obo/GAZ_00118173">
        <obo:RO_0001025 rdf:resource="http://purl.obolibrary.org/obo/GAZ_00022428"/>
        <obo:IAO_0000115>A Local-Level Government of Komo-Magarima District.</obo:IAO_0000115>
        <oboInOwl:hasOBONamespace>GAZ</oboInOwl:hasOBONamespace>
        <oboInOwl:id>GAZ:00118173</oboInOwl:id>
        <rdfs:label>Hulia Rural Local-Level Government Area</rdfs:label>
    </owl:NamedIndividual>
    


    <!-- http://purl.obolibrary.org/obo/GAZ_00118174 -->

    <owl:NamedIndividual rdf:about="http://purl.obolibrary.org/obo/GAZ_00118174">
        <obo:RO_0001025 rdf:resource="http://purl.obolibrary.org/obo/GAZ_00022428"/>
        <obo:IAO_0000115>A Local-Level Government of Komo-Magarima District.</obo:IAO_0000115>
        <oboInOwl:hasOBONamespace>GAZ</oboInOwl:hasOBONamespace>
        <oboInOwl:id>GAZ:00118174</oboInOwl:id>
        <rdfs:label>Komo Rural Local-Level Government Area</rdfs:label>
    </owl:NamedIndividual>
    


    <!-- http://purl.obolibrary.org/obo/GAZ_00118175 -->

    <owl:NamedIndividual rdf:about="http://purl.obolibrary.org/obo/GAZ_00118175">
        <obo:RO_0001025 rdf:resource="http://purl.obolibrary.org/obo/GAZ_00022428"/>
        <obo:IAO_0000115>A Local-Level Government of Komo-Magarima District.</obo:IAO_0000115>
        <oboInOwl:hasOBONamespace>GAZ</oboInOwl:hasOBONamespace>
        <oboInOwl:id>GAZ:00118175</oboInOwl:id>
        <rdfs:label>Margarima Rural Local-Level Government Area</rdfs:label>
    </owl:NamedIndividual>
    


    <!-- http://purl.obolibrary.org/obo/GAZ_00118176 -->

    <owl:NamedIndividual rdf:about="http://purl.obolibrary.org/obo/GAZ_00118176">
        <obo:RO_0001025 rdf:resource="http://purl.obolibrary.org/obo/GAZ_00022440"/>
        <obo:IAO_0000115>A Local-Level Government of Koroba-Kopiago District.</obo:IAO_0000115>
        <oboInOwl:hasOBONamespace>GAZ</oboInOwl:hasOBONamespace>
        <oboInOwl:id>GAZ:00118176</oboInOwl:id>
        <rdfs:label>Awi-Pori Rural Local-Level Government Area</rdfs:label>
    </owl:NamedIndividual>
    


    <!-- http://purl.obolibrary.org/obo/GAZ_00118177 -->

    <owl:NamedIndividual rdf:about="http://purl.obolibrary.org/obo/GAZ_00118177">
        <obo:RO_0001025 rdf:resource="http://purl.obolibrary.org/obo/GAZ_00022440"/>
        <obo:IAO_0000115>A Local-Level Government of Koroba-Kopiago District.</obo:IAO_0000115>
        <oboInOwl:hasOBONamespace>GAZ</oboInOwl:hasOBONamespace>
        <oboInOwl:id>GAZ:00118177</oboInOwl:id>
        <rdfs:label>Lake Kopiago Rural Local-Level Government Area</rdfs:label>
    </owl:NamedIndividual>
    


    <!-- http://purl.obolibrary.org/obo/GAZ_00118178 -->

    <owl:NamedIndividual rdf:about="http://purl.obolibrary.org/obo/GAZ_00118178">
        <obo:RO_0001025 rdf:resource="http://purl.obolibrary.org/obo/GAZ_00022440"/>
        <obo:IAO_0000115>A Local-Level Government of Koroba-Kopiago District.</obo:IAO_0000115>
        <oboInOwl:hasOBONamespace>GAZ</oboInOwl:hasOBONamespace>
        <oboInOwl:id>GAZ:00118178</oboInOwl:id>
        <rdfs:label>South Koroba Rural Local-Level Government Area</rdfs:label>
    </owl:NamedIndividual>
    


    <!-- http://purl.obolibrary.org/obo/GAZ_00118179 -->

    <owl:NamedIndividual rdf:about="http://purl.obolibrary.org/obo/GAZ_00118179">
        <obo:RO_0001025 rdf:resource="http://purl.obolibrary.org/obo/GAZ_00022440"/>
        <obo:IAO_0000115>A Local-Level Government of Koroba-Kopiago District.</obo:IAO_0000115>
        <oboInOwl:hasOBONamespace>GAZ</oboInOwl:hasOBONamespace>
        <oboInOwl:id>GAZ:00118179</oboInOwl:id>
        <rdfs:label>North Koroba Rural Local-Level Government Area</rdfs:label>
    </owl:NamedIndividual>
    


    <!-- http://purl.obolibrary.org/obo/GAZ_00118180 -->

    <owl:NamedIndividual rdf:about="http://purl.obolibrary.org/obo/GAZ_00118180">
        <obo:RO_0001025 rdf:resource="http://purl.obolibrary.org/obo/GAZ_00022439"/>
        <obo:IAO_0000115>A Local-Level Government of Mendi-Munihu District.</obo:IAO_0000115>
        <oboInOwl:hasOBONamespace>GAZ</oboInOwl:hasOBONamespace>
        <oboInOwl:id>GAZ:00118180</oboInOwl:id>
        <rdfs:label>Lai Valley Rural Local-Level Government Area</rdfs:label>
    </owl:NamedIndividual>
    


    <!-- http://purl.obolibrary.org/obo/GAZ_00118181 -->

    <owl:NamedIndividual rdf:about="http://purl.obolibrary.org/obo/GAZ_00118181">
        <obo:RO_0001025 rdf:resource="http://purl.obolibrary.org/obo/GAZ_00022439"/>
        <obo:IAO_0000115>A Local-Level Government of Mendi-Munihu District.</obo:IAO_0000115>
        <oboInOwl:hasOBONamespace>GAZ</oboInOwl:hasOBONamespace>
        <oboInOwl:id>GAZ:00118181</oboInOwl:id>
        <rdfs:label>Karints Rural Local-Level Government Area</rdfs:label>
    </owl:NamedIndividual>
    


    <!-- http://purl.obolibrary.org/obo/GAZ_00118182 -->

    <owl:NamedIndividual rdf:about="http://purl.obolibrary.org/obo/GAZ_00118182">
        <obo:RO_0001025 rdf:resource="http://purl.obolibrary.org/obo/GAZ_00022439"/>
        <obo:IAO_0000115>A Local-Level Government of Mendi-Munihu District.</obo:IAO_0000115>
        <oboInOwl:hasOBONamespace>GAZ</oboInOwl:hasOBONamespace>
        <oboInOwl:id>GAZ:00118182</oboInOwl:id>
        <rdfs:label>Upper Mendi Rural Local-Level Government Area</rdfs:label>
    </owl:NamedIndividual>
    


    <!-- http://purl.obolibrary.org/obo/GAZ_00118183 -->

    <owl:NamedIndividual rdf:about="http://purl.obolibrary.org/obo/GAZ_00118183">
        <obo:RO_0001025 rdf:resource="http://purl.obolibrary.org/obo/GAZ_00022439"/>
        <obo:IAO_0000115>A Local-Level Government of Mendi-Munihu District.</obo:IAO_0000115>
        <oboInOwl:hasOBONamespace>GAZ</oboInOwl:hasOBONamespace>
        <oboInOwl:id>GAZ:00118183</oboInOwl:id>
        <rdfs:label>Mendi Urban Local-Level Government Area</rdfs:label>
    </owl:NamedIndividual>
    


    <!-- http://purl.obolibrary.org/obo/GAZ_00118184 -->

    <owl:NamedIndividual rdf:about="http://purl.obolibrary.org/obo/GAZ_00118184">
        <obo:RO_0001025 rdf:resource="http://purl.obolibrary.org/obo/GAZ_00022434"/>
        <obo:IAO_0000115>A Local-Level Government of Nipa-Kutubu District.</obo:IAO_0000115>
        <oboInOwl:hasOBONamespace>GAZ</oboInOwl:hasOBONamespace>
        <oboInOwl:id>GAZ:00118184</oboInOwl:id>
        <rdfs:label>Lake Kutubu Rural Local-Level Government Area</rdfs:label>
    </owl:NamedIndividual>
    


    <!-- http://purl.obolibrary.org/obo/GAZ_00118185 -->

    <owl:NamedIndividual rdf:about="http://purl.obolibrary.org/obo/GAZ_00118185">
        <obo:RO_0001025 rdf:resource="http://purl.obolibrary.org/obo/GAZ_00022434"/>
        <obo:IAO_0000115>A Local-Level Government of Nipa-Kutubu District.</obo:IAO_0000115>
        <oboInOwl:hasOBONamespace>GAZ</oboInOwl:hasOBONamespace>
        <oboInOwl:id>GAZ:00118185</oboInOwl:id>
        <rdfs:label>Nipa Rural Local-Level Government Area</rdfs:label>
    </owl:NamedIndividual>
    


    <!-- http://purl.obolibrary.org/obo/GAZ_00118186 -->

    <owl:NamedIndividual rdf:about="http://purl.obolibrary.org/obo/GAZ_00118186">
        <obo:RO_0001025 rdf:resource="http://purl.obolibrary.org/obo/GAZ_00022434"/>
        <obo:IAO_0000115>A Local-Level Government of Nipa-Kutubu District.</obo:IAO_0000115>
        <oboInOwl:hasOBONamespace>GAZ</oboInOwl:hasOBONamespace>
        <oboInOwl:id>GAZ:00118186</oboInOwl:id>
        <rdfs:label>Poroma Rural Local-Level Government Area</rdfs:label>
    </owl:NamedIndividual>
    


    <!-- http://purl.obolibrary.org/obo/GAZ_00118187 -->

    <owl:NamedIndividual rdf:about="http://purl.obolibrary.org/obo/GAZ_00118187">
        <obo:RO_0001025 rdf:resource="http://purl.obolibrary.org/obo/GAZ_00022434"/>
        <obo:IAO_0000115>A Local-Level Government of Nipa-Kutubu District.</obo:IAO_0000115>
        <oboInOwl:hasOBONamespace>GAZ</oboInOwl:hasOBONamespace>
        <oboInOwl:id>GAZ:00118187</oboInOwl:id>
        <rdfs:label>Mount Bosavi Rural Local-Level Government Area</rdfs:label>
    </owl:NamedIndividual>
    


    <!-- http://purl.obolibrary.org/obo/GAZ_00118188 -->

    <owl:NamedIndividual rdf:about="http://purl.obolibrary.org/obo/GAZ_00118188">
        <obo:RO_0001025 rdf:resource="http://purl.obolibrary.org/obo/GAZ_00022434"/>
        <obo:IAO_0000115>A Local-Level Government of Nipa-Kutubu District.</obo:IAO_0000115>
        <oboInOwl:hasOBONamespace>GAZ</oboInOwl:hasOBONamespace>
        <oboInOwl:id>GAZ:00118188</oboInOwl:id>
        <rdfs:label>Nembi Plateau Rural Local-Level Government Area</rdfs:label>
    </owl:NamedIndividual>
    


    <!-- http://purl.obolibrary.org/obo/GAZ_00118189 -->

    <owl:NamedIndividual rdf:about="http://purl.obolibrary.org/obo/GAZ_00118189">
        <obo:RO_0001025 rdf:resource="http://purl.obolibrary.org/obo/GAZ_00022435"/>
        <obo:IAO_0000115>A Local-Level Government of Tari-Pori District.</obo:IAO_0000115>
        <oboInOwl:hasOBONamespace>GAZ</oboInOwl:hasOBONamespace>
        <oboInOwl:id>GAZ:00118189</oboInOwl:id>
        <rdfs:label>Tagali Rural Local-Level Government Area</rdfs:label>
    </owl:NamedIndividual>
    


    <!-- http://purl.obolibrary.org/obo/GAZ_00118190 -->

    <owl:NamedIndividual rdf:about="http://purl.obolibrary.org/obo/GAZ_00118190">
        <obo:RO_0001025 rdf:resource="http://purl.obolibrary.org/obo/GAZ_00022435"/>
        <obo:IAO_0000115>A Local-Level Government of Tari-Pori District.</obo:IAO_0000115>
        <oboInOwl:hasOBONamespace>GAZ</oboInOwl:hasOBONamespace>
        <oboInOwl:id>GAZ:00118190</oboInOwl:id>
        <rdfs:label>Tari Urban Local-Level Government Area</rdfs:label>
    </owl:NamedIndividual>
    


    <!-- http://purl.obolibrary.org/obo/GAZ_00118191 -->

    <owl:NamedIndividual rdf:about="http://purl.obolibrary.org/obo/GAZ_00118191">
        <obo:RO_0001025 rdf:resource="http://purl.obolibrary.org/obo/GAZ_00022435"/>
        <obo:IAO_0000115>A Local-Level Government of Tari-Pori District.</obo:IAO_0000115>
        <oboInOwl:hasOBONamespace>GAZ</oboInOwl:hasOBONamespace>
        <oboInOwl:id>GAZ:00118191</oboInOwl:id>
        <rdfs:label>Tebi Rural Local-Level Government Area</rdfs:label>
    </owl:NamedIndividual>
    


    <!-- http://purl.obolibrary.org/obo/GAZ_00118192 -->

    <owl:NamedIndividual rdf:about="http://purl.obolibrary.org/obo/GAZ_00118192">
        <obo:RO_0001025 rdf:resource="http://purl.obolibrary.org/obo/GAZ_00022435"/>
        <obo:IAO_0000115>A Local-Level Government of Tari-Pori District.</obo:IAO_0000115>
        <oboInOwl:hasOBONamespace>GAZ</oboInOwl:hasOBONamespace>
        <oboInOwl:id>GAZ:00118192</oboInOwl:id>
        <rdfs:label>Hayapuga Rural Local-Level Government Area</rdfs:label>
    </owl:NamedIndividual>
    


    <!-- http://purl.obolibrary.org/obo/GAZ_00118193 -->

    <owl:NamedIndividual rdf:about="http://purl.obolibrary.org/obo/GAZ_00118193">
        <obo:RO_0001025 rdf:resource="http://purl.obolibrary.org/obo/GAZ_00022421"/>
        <obo:IAO_0000115>A Local-Level Government Area of Anglimp-South Waghi District.</obo:IAO_0000115>
        <oboInOwl:hasOBONamespace>GAZ</oboInOwl:hasOBONamespace>
        <oboInOwl:id>GAZ:00118193</oboInOwl:id>
        <rdfs:label>South Waghi Rural Local-Level Government Area</rdfs:label>
    </owl:NamedIndividual>
    


    <!-- http://purl.obolibrary.org/obo/GAZ_00118194 -->

    <owl:NamedIndividual rdf:about="http://purl.obolibrary.org/obo/GAZ_00118194">
        <obo:RO_0001025 rdf:resource="http://purl.obolibrary.org/obo/GAZ_00022421"/>
        <obo:IAO_0000115>A Local-Level Government Area of Anglimp-South Waghi District.</obo:IAO_0000115>
        <oboInOwl:hasOBONamespace>GAZ</oboInOwl:hasOBONamespace>
        <oboInOwl:id>GAZ:00118194</oboInOwl:id>
        <rdfs:label>Anglimp Rural Local-Level Government Area</rdfs:label>
    </owl:NamedIndividual>
    


    <!-- http://purl.obolibrary.org/obo/GAZ_00118195 -->

    <owl:NamedIndividual rdf:about="http://purl.obolibrary.org/obo/GAZ_00118195">
        <obo:RO_0001025 rdf:resource="http://purl.obolibrary.org/obo/GAZ_00022420"/>
        <obo:IAO_0000115>A Local-Level Government Area of Dei District.</obo:IAO_0000115>
        <oboInOwl:hasOBONamespace>GAZ</oboInOwl:hasOBONamespace>
        <oboInOwl:id>GAZ:00118195</oboInOwl:id>
        <rdfs:label>Muglamp Rural Local-Level Government Area</rdfs:label>
    </owl:NamedIndividual>
    


    <!-- http://purl.obolibrary.org/obo/GAZ_00118196 -->

    <owl:NamedIndividual rdf:about="http://purl.obolibrary.org/obo/GAZ_00118196">
        <obo:RO_0001025 rdf:resource="http://purl.obolibrary.org/obo/GAZ_00022420"/>
        <obo:IAO_0000115>A Local-Level Government Area of Dei District.</obo:IAO_0000115>
        <oboInOwl:hasOBONamespace>GAZ</oboInOwl:hasOBONamespace>
        <oboInOwl:id>GAZ:00118196</oboInOwl:id>
        <rdfs:label>Kotna Rural Local-Level Government Area</rdfs:label>
    </owl:NamedIndividual>
    


    <!-- http://purl.obolibrary.org/obo/GAZ_00118197 -->

    <owl:NamedIndividual rdf:about="http://purl.obolibrary.org/obo/GAZ_00118197">
        <obo:RO_0001025 rdf:resource="http://purl.obolibrary.org/obo/GAZ_00022425"/>
        <obo:IAO_0000115>A Local-Level Government Area of Jimi District.</obo:IAO_0000115>
        <oboInOwl:hasOBONamespace>GAZ</oboInOwl:hasOBONamespace>
        <oboInOwl:id>GAZ:00118197</oboInOwl:id>
        <rdfs:label>Jimi Rural Local-Level Government Area</rdfs:label>
    </owl:NamedIndividual>
    


    <!-- http://purl.obolibrary.org/obo/GAZ_00118198 -->

    <owl:NamedIndividual rdf:about="http://purl.obolibrary.org/obo/GAZ_00118198">
        <obo:RO_0001025 rdf:resource="http://purl.obolibrary.org/obo/GAZ_00022425"/>
        <obo:IAO_0000115>A Local-Level Government Area of Jimi District.</obo:IAO_0000115>
        <oboInOwl:hasOBONamespace>GAZ</oboInOwl:hasOBONamespace>
        <oboInOwl:id>GAZ:00118198</oboInOwl:id>
        <rdfs:label>Koi Rural Local-Level Government Area</rdfs:label>
    </owl:NamedIndividual>
    


    <!-- http://purl.obolibrary.org/obo/GAZ_00118199 -->

    <owl:NamedIndividual rdf:about="http://purl.obolibrary.org/obo/GAZ_00118199">
        <obo:RO_0001025 rdf:resource="http://purl.obolibrary.org/obo/GAZ_00022423"/>
        <obo:IAO_0000115>A Local-Level Government Area of Mount Hagen District.</obo:IAO_0000115>
        <oboInOwl:hasOBONamespace>GAZ</oboInOwl:hasOBONamespace>
        <oboInOwl:id>GAZ:00118199</oboInOwl:id>
        <rdfs:label>Mount Hagen Rural Local-Level Government Area</rdfs:label>
    </owl:NamedIndividual>
    


    <!-- http://purl.obolibrary.org/obo/GAZ_00118200 -->

    <owl:NamedIndividual rdf:about="http://purl.obolibrary.org/obo/GAZ_00118200">
        <obo:RO_0001025 rdf:resource="http://purl.obolibrary.org/obo/GAZ_00022423"/>
        <obo:IAO_0000115>A Local-Level Government Area of Mount Hagen District.</obo:IAO_0000115>
        <oboInOwl:hasOBONamespace>GAZ</oboInOwl:hasOBONamespace>
        <oboInOwl:id>GAZ:00118200</oboInOwl:id>
        <rdfs:label>Mount Hagen Urban Local-Level Government Area</rdfs:label>
    </owl:NamedIndividual>
    


    <!-- http://purl.obolibrary.org/obo/GAZ_00118201 -->

    <owl:NamedIndividual rdf:about="http://purl.obolibrary.org/obo/GAZ_00118201">
        <obo:RO_0001025 rdf:resource="http://purl.obolibrary.org/obo/GAZ_00022422"/>
        <obo:IAO_0000115>A Local-Level Government Area of Mul-Baiyer District.</obo:IAO_0000115>
        <oboInOwl:hasOBONamespace>GAZ</oboInOwl:hasOBONamespace>
        <oboInOwl:id>GAZ:00118201</oboInOwl:id>
        <rdfs:label>Baiyer Rural Local-Level Government Area</rdfs:label>
    </owl:NamedIndividual>
    


    <!-- http://purl.obolibrary.org/obo/GAZ_00118202 -->

    <owl:NamedIndividual rdf:about="http://purl.obolibrary.org/obo/GAZ_00118202">
        <obo:RO_0001025 rdf:resource="http://purl.obolibrary.org/obo/GAZ_00022422"/>
        <obo:IAO_0000115>A Local-Level Government Area of Mul-Baiyer District.</obo:IAO_0000115>
        <oboInOwl:hasOBONamespace>GAZ</oboInOwl:hasOBONamespace>
        <oboInOwl:id>GAZ:00118202</oboInOwl:id>
        <rdfs:label>Lumusa Rural Local-Level Government Area</rdfs:label>
    </owl:NamedIndividual>
    


    <!-- http://purl.obolibrary.org/obo/GAZ_00118203 -->

    <owl:NamedIndividual rdf:about="http://purl.obolibrary.org/obo/GAZ_00118203">
        <obo:RO_0001025 rdf:resource="http://purl.obolibrary.org/obo/GAZ_00022422"/>
        <obo:IAO_0000115>A Local-Level Government Area of Mul-Baiyer District.</obo:IAO_0000115>
        <oboInOwl:hasOBONamespace>GAZ</oboInOwl:hasOBONamespace>
        <oboInOwl:id>GAZ:00118203</oboInOwl:id>
        <rdfs:label>Mul Rural Local-Level Government Area</rdfs:label>
    </owl:NamedIndividual>
    


    <!-- http://purl.obolibrary.org/obo/GAZ_00118204 -->

    <owl:NamedIndividual rdf:about="http://purl.obolibrary.org/obo/GAZ_00118204">
        <obo:RO_0001025 rdf:resource="http://purl.obolibrary.org/obo/GAZ_00022426"/>
        <obo:IAO_0000115>A Local-Level Government Area of North Waghi District.</obo:IAO_0000115>
        <oboInOwl:hasOBONamespace>GAZ</oboInOwl:hasOBONamespace>
        <oboInOwl:id>GAZ:00118204</oboInOwl:id>
        <rdfs:label>North Waghi Rural Local-Level Government Area</rdfs:label>
    </owl:NamedIndividual>
    


    <!-- http://purl.obolibrary.org/obo/GAZ_00118205 -->

    <owl:NamedIndividual rdf:about="http://purl.obolibrary.org/obo/GAZ_00118205">
        <obo:RO_0001025 rdf:resource="http://purl.obolibrary.org/obo/GAZ_00022426"/>
        <obo:IAO_0000115>A Local-Level Government Area of North Waghi District.</obo:IAO_0000115>
        <oboInOwl:hasOBONamespace>GAZ</oboInOwl:hasOBONamespace>
        <oboInOwl:id>GAZ:00118205</oboInOwl:id>
        <rdfs:label>Nondugl Rural Local-Level Government Area</rdfs:label>
    </owl:NamedIndividual>
    


    <!-- http://purl.obolibrary.org/obo/GAZ_00118206 -->

    <owl:NamedIndividual rdf:about="http://purl.obolibrary.org/obo/GAZ_00118206">
        <obo:RO_0001025 rdf:resource="http://purl.obolibrary.org/obo/GAZ_00022424"/>
        <obo:IAO_0000115>A Local-Level Government Area of Tambul-Nebilyer District.</obo:IAO_0000115>
        <oboInOwl:hasOBONamespace>GAZ</oboInOwl:hasOBONamespace>
        <oboInOwl:id>GAZ:00118206</oboInOwl:id>
        <rdfs:label>Mount Giluwe Rural Local-Level Government Area</rdfs:label>
    </owl:NamedIndividual>
    


    <!-- http://purl.obolibrary.org/obo/GAZ_00118207 -->

    <owl:NamedIndividual rdf:about="http://purl.obolibrary.org/obo/GAZ_00118207">
        <obo:RO_0001025 rdf:resource="http://purl.obolibrary.org/obo/GAZ_00022424"/>
        <obo:IAO_0000115>A Local-Level Government Area of Tambul-Nebilyer District.</obo:IAO_0000115>
        <oboInOwl:hasOBONamespace>GAZ</oboInOwl:hasOBONamespace>
        <oboInOwl:id>GAZ:00118207</oboInOwl:id>
        <rdfs:label>Nebilyer Rural Local-Level Government Area</rdfs:label>
    </owl:NamedIndividual>
    


    <!-- http://purl.obolibrary.org/obo/GAZ_00118274 -->

    <owl:NamedIndividual rdf:about="http://purl.obolibrary.org/obo/GAZ_00118274">
        <obo:RO_0001025 rdf:resource="http://purl.obolibrary.org/obo/GAZ_00118095"/>
        <oboInOwl:hasOBONamespace>GAZ</oboInOwl:hasOBONamespace>
        <oboInOwl:id>GAZ:00118274</oboInOwl:id>
        <rdfs:label>Mallum Islands</rdfs:label>
    </owl:NamedIndividual>
    


    <!-- http://purl.obolibrary.org/obo/GAZ_00118275 -->

    <owl:NamedIndividual rdf:about="http://purl.obolibrary.org/obo/GAZ_00118275">
        <obo:RO_0001025 rdf:resource="http://purl.obolibrary.org/obo/GAZ_00053882"/>
        <obo:IAO_0000115>A freshwater crater lake.</obo:IAO_0000115>
        <oboInOwl:hasOBONamespace>GAZ</oboInOwl:hasOBONamespace>
        <oboInOwl:id>GAZ:00118275</oboInOwl:id>
        <rdfs:label>Lake Wisdom</rdfs:label>
    </owl:NamedIndividual>
    


    <!-- http://purl.obolibrary.org/obo/GAZ_00118276 -->

    <owl:NamedIndividual rdf:about="http://purl.obolibrary.org/obo/GAZ_00118276">
        <obo:RO_0001025 rdf:resource="http://purl.obolibrary.org/obo/GAZ_00051599"/>
        <obo:IAO_0000115>A 30 km wide stretch of water separating Papua New Guinea from Goodenough Island in the D&apos;Entrecasteaux Islands. The Dart Reefs are located in the centre of the channel.</obo:IAO_0000115>
        <oboInOwl:hasOBONamespace>GAZ</oboInOwl:hasOBONamespace>
        <oboInOwl:id>GAZ:00118276</oboInOwl:id>
        <rdfs:label>Ward Hunt Strait</rdfs:label>
    </owl:NamedIndividual>
    


    <!-- http://purl.obolibrary.org/obo/GAZ_00118277 -->

    <owl:NamedIndividual rdf:about="http://purl.obolibrary.org/obo/GAZ_00118277">
        <obo:RO_0001025 rdf:resource="http://purl.obolibrary.org/obo/GAZ_00118276"/>
        <obo:IAO_0000115>A collective of reefs in the central area of the Ward Hunt Strait. The reefs are ribbon-like structured patch reefs. They are located approximately 15 km from Papua New Guinea and the same distance from the island of Goodenough in the D&apos;Entrecasteaux Islands.</obo:IAO_0000115>
        <oboInOwl:hasOBONamespace>GAZ</oboInOwl:hasOBONamespace>
        <oboInOwl:id>GAZ:00118277</oboInOwl:id>
        <rdfs:label>Dart Reefs</rdfs:label>
    </owl:NamedIndividual>
    


    <!-- http://purl.obolibrary.org/obo/GAZ_00118278 -->

    <owl:NamedIndividual rdf:about="http://purl.obolibrary.org/obo/GAZ_00118278">
        <obo:RO_0001025 rdf:resource="http://purl.obolibrary.org/obo/GAZ_00118366"/>
        <obo:IAO_0000115>One of the Green Islands.</obo:IAO_0000115>
        <oboInOwl:hasOBONamespace>GAZ</oboInOwl:hasOBONamespace>
        <oboInOwl:id>GAZ:00118278</oboInOwl:id>
        <rdfs:label>Sirot Island</rdfs:label>
    </owl:NamedIndividual>
    


    <!-- http://purl.obolibrary.org/obo/GAZ_00118279 -->

    <owl:NamedIndividual rdf:about="http://purl.obolibrary.org/obo/GAZ_00118279">
        <obo:RO_0001025 rdf:resource="http://purl.obolibrary.org/obo/GAZ_00118366"/>
        <obo:IAO_0000115>One of the Green Islands.</obo:IAO_0000115>
        <oboInOwl:hasOBONamespace>GAZ</oboInOwl:hasOBONamespace>
        <oboInOwl:id>GAZ:00118279</oboInOwl:id>
        <rdfs:label>Barahun Island</rdfs:label>
    </owl:NamedIndividual>
    


    <!-- http://purl.obolibrary.org/obo/GAZ_00118280 -->

    <owl:NamedIndividual rdf:about="http://purl.obolibrary.org/obo/GAZ_00118280">
        <obo:RO_0001025 rdf:resource="http://purl.obolibrary.org/obo/GAZ_00118363"/>
        <obo:IAO_0000115>One of the Green Islands.</obo:IAO_0000115>
        <oboInOwl:hasOBONamespace>GAZ</oboInOwl:hasOBONamespace>
        <oboInOwl:id>GAZ:00118280</oboInOwl:id>
        <rdfs:label>Pinipel Island</rdfs:label>
    </owl:NamedIndividual>
    


    <!-- http://purl.obolibrary.org/obo/GAZ_00118282 -->

    <owl:NamedIndividual rdf:about="http://purl.obolibrary.org/obo/GAZ_00118282">
        <obo:RO_0001025 rdf:resource="http://purl.obolibrary.org/obo/GAZ_00118366"/>
        <obo:IAO_0000115>The largest of the Green Islands of Papua New Guinea.</obo:IAO_0000115>
        <oboInOwl:hasOBONamespace>GAZ</oboInOwl:hasOBONamespace>
        <oboInOwl:id>GAZ:00118282</oboInOwl:id>
        <rdfs:label>Nissan Island</rdfs:label>
    </owl:NamedIndividual>
    


    <!-- http://purl.obolibrary.org/obo/GAZ_00118283 -->

    <owl:NamedIndividual rdf:about="http://purl.obolibrary.org/obo/GAZ_00118283">
        <obo:RO_0001025 rdf:resource="http://purl.obolibrary.org/obo/GAZ_00051599"/>
        <obo:IAO_0000115>An island in Milne Bay.</obo:IAO_0000115>
        <oboInOwl:hasOBONamespace>GAZ</oboInOwl:hasOBONamespace>
        <oboInOwl:id>GAZ:00118283</oboInOwl:id>
        <rdfs:label>Hemenahei Island</rdfs:label>
    </owl:NamedIndividual>
    


    <!-- http://purl.obolibrary.org/obo/GAZ_00118284 -->

    <owl:NamedIndividual rdf:about="http://purl.obolibrary.org/obo/GAZ_00118284">
        <obo:RO_0001025 rdf:resource="http://purl.obolibrary.org/obo/GAZ_00012665"/>
        <obo:IAO_0000115>The second longest river, after the Sepik, in Papua New Guinea. It rises in the Star Mountains, and crosses the south-western lowlands before flowing into the Gulf of Papua in a large delta. It flows mostly through the Western Province, though for a small stretch it forms the boundary between PNG and the Indonesia province of Papua.</obo:IAO_0000115>
        <oboInOwl:hasOBONamespace>GAZ</oboInOwl:hasOBONamespace>
        <oboInOwl:id>GAZ:00118284</oboInOwl:id>
        <rdfs:label>Fly River</rdfs:label>
    </owl:NamedIndividual>
    


    <!-- http://purl.obolibrary.org/obo/GAZ_00118285 -->

    <owl:NamedIndividual rdf:about="http://purl.obolibrary.org/obo/GAZ_00118285">
        <obo:RO_0001025 rdf:resource="http://purl.obolibrary.org/obo/GAZ_00118284"/>
        <obo:IAO_0000115>The delta of the Fly River.</obo:IAO_0000115>
        <oboInOwl:hasOBONamespace>GAZ</oboInOwl:hasOBONamespace>
        <oboInOwl:id>GAZ:00118285</oboInOwl:id>
        <rdfs:label>Fly River Delta</rdfs:label>
    </owl:NamedIndividual>
    


    <!-- http://purl.obolibrary.org/obo/GAZ_00118286 -->

    <owl:NamedIndividual rdf:about="http://purl.obolibrary.org/obo/GAZ_00118286">
        <obo:RO_0001025 rdf:resource="http://purl.obolibrary.org/obo/GAZ_00118285"/>
        <obo:IAO_0000115>An island in the Fly River delta, Papua New Guinea.</obo:IAO_0000115>
        <oboInOwl:hasOBONamespace>GAZ</oboInOwl:hasOBONamespace>
        <oboInOwl:id>GAZ:00118286</oboInOwl:id>
        <rdfs:label>Kiwai Island</rdfs:label>
    </owl:NamedIndividual>
    


    <!-- http://purl.obolibrary.org/obo/GAZ_00118287 -->

    <owl:NamedIndividual rdf:about="http://purl.obolibrary.org/obo/GAZ_00118287">
        <obo:RO_0001025 rdf:resource="http://purl.obolibrary.org/obo/GAZ_00051599"/>
        <obo:IAO_0000115>An island in Milne Bay.</obo:IAO_0000115>
        <oboInOwl:hasOBONamespace>GAZ</oboInOwl:hasOBONamespace>
        <oboInOwl:id>GAZ:00118287</oboInOwl:id>
        <rdfs:label>Madau Island</rdfs:label>
    </owl:NamedIndividual>
    


    <!-- http://purl.obolibrary.org/obo/GAZ_00118288 -->

    <owl:NamedIndividual rdf:about="http://purl.obolibrary.org/obo/GAZ_00118288">
        <obo:RO_0001025 rdf:resource="http://purl.obolibrary.org/obo/GAZ_00051589"/>
        <obo:IAO_0000115>One of the Marshall Bennett Islands.</obo:IAO_0000115>
        <oboInOwl:hasOBONamespace>GAZ</oboInOwl:hasOBONamespace>
        <oboInOwl:id>GAZ:00118288</oboInOwl:id>
        <rdfs:label>Nagian Island</rdfs:label>
    </owl:NamedIndividual>
    


    <!-- http://purl.obolibrary.org/obo/GAZ_00118289 -->

    <owl:NamedIndividual rdf:about="http://purl.obolibrary.org/obo/GAZ_00118289">
        <obo:RO_0001025 rdf:resource="http://purl.obolibrary.org/obo/GAZ_00051589"/>
        <obo:IAO_0000115>One of the Marshall Bennett Islands.</obo:IAO_0000115>
        <oboInOwl:hasOBONamespace>GAZ</oboInOwl:hasOBONamespace>
        <oboInOwl:id>GAZ:00118289</oboInOwl:id>
        <rdfs:label>Wiakau Island</rdfs:label>
    </owl:NamedIndividual>
    


    <!-- http://purl.obolibrary.org/obo/GAZ_00118290 -->

    <owl:NamedIndividual rdf:about="http://purl.obolibrary.org/obo/GAZ_00118290">
        <obo:RO_0001025 rdf:resource="http://purl.obolibrary.org/obo/GAZ_00051589"/>
        <obo:IAO_0000115>One of the Marshall Bennett Islands.</obo:IAO_0000115>
        <oboInOwl:hasOBONamespace>GAZ</oboInOwl:hasOBONamespace>
        <oboInOwl:id>GAZ:00118290</oboInOwl:id>
        <rdfs:label>Yanaba Island</rdfs:label>
    </owl:NamedIndividual>
    


    <!-- http://purl.obolibrary.org/obo/GAZ_00118291 -->

    <owl:NamedIndividual rdf:about="http://purl.obolibrary.org/obo/GAZ_00118291">
        <obo:RO_0001025 rdf:resource="http://purl.obolibrary.org/obo/GAZ_00051599"/>
        <obo:IAO_0000115>A 12-18 km wide stretch of water that separates Normanby Island from the New Guinea mainland and from the numerous reefs and islands the line the entrance into Milne Bay.</obo:IAO_0000115>
        <oboInOwl:hasOBONamespace>GAZ</oboInOwl:hasOBONamespace>
        <oboInOwl:id>GAZ:00118291</oboInOwl:id>
        <rdfs:label>Goschen Strait</rdfs:label>
    </owl:NamedIndividual>
    


    <!-- http://purl.obolibrary.org/obo/GAZ_00118292 -->

    <owl:NamedIndividual rdf:about="http://purl.obolibrary.org/obo/GAZ_00118292">
        <obo:RO_0001025 rdf:resource="http://purl.obolibrary.org/obo/GAZ_00118291"/>
        <obo:IAO_0000115>A small, mountainous island in the Goschen Strait south of Normanby Island and east of East Cape. It is part of Milne Bay Province, Papua New Guinea.</obo:IAO_0000115>
        <oboInOwl:hasOBONamespace>GAZ</oboInOwl:hasOBONamespace>
        <oboInOwl:id>GAZ:00118292</oboInOwl:id>
        <rdfs:label>Nuakata Island</rdfs:label>
    </owl:NamedIndividual>
    


    <!-- http://purl.obolibrary.org/obo/GAZ_00118293 -->

    <owl:NamedIndividual rdf:about="http://purl.obolibrary.org/obo/GAZ_00118293">
        <obo:RO_0001025 rdf:resource="http://purl.obolibrary.org/obo/GAZ_00007182"/>
        <obo:IAO_0000115>An island in the Louisiade Archipelago in Milne Bay Province, Papua New Guinea.</obo:IAO_0000115>
        <oboInOwl:hasOBONamespace>GAZ</oboInOwl:hasOBONamespace>
        <oboInOwl:id>GAZ:00118293</oboInOwl:id>
        <rdfs:label>Pana Tinai</rdfs:label>
    </owl:NamedIndividual>
    


    <!-- http://purl.obolibrary.org/obo/GAZ_00118294 -->

    <owl:NamedIndividual rdf:about="http://purl.obolibrary.org/obo/GAZ_00118294">
        <obo:RO_0001025 rdf:resource="http://purl.obolibrary.org/obo/GAZ_00051599"/>
        <obo:RO_0001025 rdf:resource="http://purl.obolibrary.org/obo/GAZ_00118045"/>
        <obo:IAO_0000115>A coral reef and a mostly submerged atoll in the far southeast of Papua New Guinea. It is 162.4 km from the closest island, Loa Boloba, which is a tiny coral islet within the fringing reef near Cape Deliverance, the south east point of Rossel Island (Yela) in the Louisiade Archipelago, and belongs to Milne Bay province, Samarai-Murua District, Louisiade Rural Local Level Government Area. Pocklington Reef sits on top of Pocklington Ridge, which extends northeast from Rossel Island. The reef is 32 km long and up to 4 km wide. Its longer axis is northeast-southwest. The rim of the reef encloses a deep lagoon. The northern rim reaches closer to the surface, and several above water rocks with heights between 0.9 and 3 meters high lie along its length. There is a small spit of sand about the size of a football field at the northeast end.</obo:IAO_0000115>
        <oboInOwl:hasOBONamespace>GAZ</oboInOwl:hasOBONamespace>
        <oboInOwl:id>GAZ:00118294</oboInOwl:id>
        <rdfs:label>Pocklington Reef</rdfs:label>
    </owl:NamedIndividual>
    


    <!-- http://purl.obolibrary.org/obo/GAZ_00118295 -->

    <owl:NamedIndividual rdf:about="http://purl.obolibrary.org/obo/GAZ_00118295">
        <obo:RO_0001025 rdf:resource="http://purl.obolibrary.org/obo/GAZ_00118285"/>
        <obo:IAO_0000115>An island in the Fly River delta, Papua New Guinea.</obo:IAO_0000115>
        <oboInOwl:hasOBONamespace>GAZ</oboInOwl:hasOBONamespace>
        <oboInOwl:id>GAZ:00118295</oboInOwl:id>
        <rdfs:label>Purutu Island</rdfs:label>
    </owl:NamedIndividual>
    


    <!-- http://purl.obolibrary.org/obo/GAZ_00118296 -->

    <owl:NamedIndividual rdf:about="http://purl.obolibrary.org/obo/GAZ_00118296">
        <obo:RO_0001025 rdf:resource="http://purl.obolibrary.org/obo/GAZ_00118285"/>
        <obo:IAO_0000115>An island in the Fly River delta, Papua New Guinea.</obo:IAO_0000115>
        <oboInOwl:hasOBONamespace>GAZ</oboInOwl:hasOBONamespace>
        <oboInOwl:id>GAZ:00118296</oboInOwl:id>
        <rdfs:label>Wabuda Island</rdfs:label>
    </owl:NamedIndividual>
    


    <!-- http://purl.obolibrary.org/obo/GAZ_00118297 -->

    <owl:NamedIndividual rdf:about="http://purl.obolibrary.org/obo/GAZ_00118297">
        <obo:RO_0001025 rdf:resource="http://purl.obolibrary.org/obo/GAZ_00007183"/>
        <obo:IAO_0000115>One of the Trobriand Islands.</obo:IAO_0000115>
        <oboInOwl:hasOBONamespace>GAZ</oboInOwl:hasOBONamespace>
        <oboInOwl:id>GAZ:00118297</oboInOwl:id>
        <rdfs:label>Kuaniagal Island</rdfs:label>
    </owl:NamedIndividual>
    


    <!-- http://purl.obolibrary.org/obo/GAZ_00118298 -->

    <owl:NamedIndividual rdf:about="http://purl.obolibrary.org/obo/GAZ_00118298">
        <obo:RO_0001025 rdf:resource="http://purl.obolibrary.org/obo/GAZ_00007183"/>
        <obo:IAO_0000115>One of the Trobriand Islands.</obo:IAO_0000115>
        <oboInOwl:hasOBONamespace>GAZ</oboInOwl:hasOBONamespace>
        <oboInOwl:id>GAZ:00118298</oboInOwl:id>
        <rdfs:label>Gabwina Island</rdfs:label>
    </owl:NamedIndividual>
    


    <!-- http://purl.obolibrary.org/obo/GAZ_00118299 -->

    <owl:NamedIndividual rdf:about="http://purl.obolibrary.org/obo/GAZ_00118299">
        <obo:RO_0001025 rdf:resource="http://purl.obolibrary.org/obo/GAZ_00007183"/>
        <obo:IAO_0000115>One of the Trobriand Islands.</obo:IAO_0000115>
        <oboInOwl:hasOBONamespace>GAZ</oboInOwl:hasOBONamespace>
        <oboInOwl:id>GAZ:00118299</oboInOwl:id>
        <rdfs:label>Gwadarab Island</rdfs:label>
    </owl:NamedIndividual>
    


    <!-- http://purl.obolibrary.org/obo/GAZ_00118300 -->

    <owl:NamedIndividual rdf:about="http://purl.obolibrary.org/obo/GAZ_00118300">
        <obo:RO_0001025 rdf:resource="http://purl.obolibrary.org/obo/GAZ_00007183"/>
        <obo:IAO_0000115>One of the Trobriand Islands.</obo:IAO_0000115>
        <oboInOwl:hasOBONamespace>GAZ</oboInOwl:hasOBONamespace>
        <oboInOwl:id>GAZ:00118300</oboInOwl:id>
        <rdfs:label>Konokonowana Island</rdfs:label>
    </owl:NamedIndividual>
    


    <!-- http://purl.obolibrary.org/obo/GAZ_00118301 -->

    <owl:NamedIndividual rdf:about="http://purl.obolibrary.org/obo/GAZ_00118301">
        <obo:RO_0001025 rdf:resource="http://purl.obolibrary.org/obo/GAZ_00007183"/>
        <obo:IAO_0000115>One of the Trobriand Islands.</obo:IAO_0000115>
        <oboInOwl:hasOBONamespace>GAZ</oboInOwl:hasOBONamespace>
        <oboInOwl:id>GAZ:00118301</oboInOwl:id>
        <rdfs:label>Kanupa Island</rdfs:label>
    </owl:NamedIndividual>
    


    <!-- http://purl.obolibrary.org/obo/GAZ_00118302 -->

    <owl:NamedIndividual rdf:about="http://purl.obolibrary.org/obo/GAZ_00118302">
        <obo:RO_0001025 rdf:resource="http://purl.obolibrary.org/obo/GAZ_00007183"/>
        <obo:IAO_0000115>One of the Trobriand Islands.</obo:IAO_0000115>
        <oboInOwl:hasOBONamespace>GAZ</oboInOwl:hasOBONamespace>
        <oboInOwl:id>GAZ:00118302</oboInOwl:id>
        <rdfs:label>Lulima Island</rdfs:label>
    </owl:NamedIndividual>
    


    <!-- http://purl.obolibrary.org/obo/GAZ_00118303 -->

    <owl:NamedIndividual rdf:about="http://purl.obolibrary.org/obo/GAZ_00118303">
        <obo:RO_0001025 rdf:resource="http://purl.obolibrary.org/obo/GAZ_00007183"/>
        <obo:IAO_0000115>One of the Trobriand Islands.</obo:IAO_0000115>
        <oboInOwl:hasOBONamespace>GAZ</oboInOwl:hasOBONamespace>
        <oboInOwl:id>GAZ:00118303</oboInOwl:id>
        <rdfs:label>Deia Island</rdfs:label>
    </owl:NamedIndividual>
    


    <!-- http://purl.obolibrary.org/obo/GAZ_00118304 -->

    <owl:NamedIndividual rdf:about="http://purl.obolibrary.org/obo/GAZ_00118304">
        <obo:RO_0001025 rdf:resource="http://purl.obolibrary.org/obo/GAZ_00007183"/>
        <obo:IAO_0000115>One of the Trobriand Islands.</obo:IAO_0000115>
        <oboInOwl:hasOBONamespace>GAZ</oboInOwl:hasOBONamespace>
        <oboInOwl:id>GAZ:00118304</oboInOwl:id>
        <rdfs:label>Simsim Island</rdfs:label>
    </owl:NamedIndividual>
    


    <!-- http://purl.obolibrary.org/obo/GAZ_00118305 -->

    <owl:NamedIndividual rdf:about="http://purl.obolibrary.org/obo/GAZ_00118305">
        <obo:RO_0001025 rdf:resource="http://purl.obolibrary.org/obo/GAZ_00007183"/>
        <obo:IAO_0000115>One of the Trobriand Islands.</obo:IAO_0000115>
        <oboInOwl:hasOBONamespace>GAZ</oboInOwl:hasOBONamespace>
        <oboInOwl:id>GAZ:00118305</oboInOwl:id>
        <rdfs:label>Nuarguta Island</rdfs:label>
    </owl:NamedIndividual>
    


    <!-- http://purl.obolibrary.org/obo/GAZ_00118306 -->

    <owl:NamedIndividual rdf:about="http://purl.obolibrary.org/obo/GAZ_00118306">
        <obo:RO_0001025 rdf:resource="http://purl.obolibrary.org/obo/GAZ_00007183"/>
        <obo:IAO_0000115>One of the Trobriand Islands.</obo:IAO_0000115>
        <oboInOwl:hasOBONamespace>GAZ</oboInOwl:hasOBONamespace>
        <oboInOwl:id>GAZ:00118306</oboInOwl:id>
        <rdfs:label>Simlindon Island</rdfs:label>
    </owl:NamedIndividual>
    


    <!-- http://purl.obolibrary.org/obo/GAZ_00118307 -->

    <owl:NamedIndividual rdf:about="http://purl.obolibrary.org/obo/GAZ_00118307">
        <obo:RO_0001025 rdf:resource="http://purl.obolibrary.org/obo/GAZ_00007183"/>
        <obo:IAO_0000115>One of the Trobriand Islands.</obo:IAO_0000115>
        <oboInOwl:hasOBONamespace>GAZ</oboInOwl:hasOBONamespace>
        <oboInOwl:id>GAZ:00118307</oboInOwl:id>
        <rdfs:label>Wagalasa Island</rdfs:label>
    </owl:NamedIndividual>
    


    <!-- http://purl.obolibrary.org/obo/GAZ_00118308 -->

    <owl:NamedIndividual rdf:about="http://purl.obolibrary.org/obo/GAZ_00118308">
        <obo:RO_0001025 rdf:resource="http://purl.obolibrary.org/obo/GAZ_00007183"/>
        <obo:IAO_0000115>One of the Trobriand Islands.</obo:IAO_0000115>
        <oboInOwl:hasOBONamespace>GAZ</oboInOwl:hasOBONamespace>
        <oboInOwl:id>GAZ:00118308</oboInOwl:id>
        <rdfs:label>Siliniaka Island</rdfs:label>
    </owl:NamedIndividual>
    


    <!-- http://purl.obolibrary.org/obo/GAZ_00118309 -->

    <owl:NamedIndividual rdf:about="http://purl.obolibrary.org/obo/GAZ_00118309">
        <obo:RO_0001025 rdf:resource="http://purl.obolibrary.org/obo/GAZ_00007183"/>
        <obo:IAO_0000115>One of the Trobriand Islands.</obo:IAO_0000115>
        <oboInOwl:hasOBONamespace>GAZ</oboInOwl:hasOBONamespace>
        <oboInOwl:id>GAZ:00118309</oboInOwl:id>
        <rdfs:label>Kawa Island</rdfs:label>
    </owl:NamedIndividual>
    


    <!-- http://purl.obolibrary.org/obo/GAZ_00118310 -->

    <owl:NamedIndividual rdf:about="http://purl.obolibrary.org/obo/GAZ_00118310">
        <obo:RO_0001025 rdf:resource="http://purl.obolibrary.org/obo/GAZ_00007183"/>
        <obo:IAO_0000115>One of the Trobriand Islands.</obo:IAO_0000115>
        <oboInOwl:hasOBONamespace>GAZ</oboInOwl:hasOBONamespace>
        <oboInOwl:id>GAZ:00118310</oboInOwl:id>
        <rdfs:label>Nauria Island</rdfs:label>
    </owl:NamedIndividual>
    


    <!-- http://purl.obolibrary.org/obo/GAZ_00118311 -->

    <owl:NamedIndividual rdf:about="http://purl.obolibrary.org/obo/GAZ_00118311">
        <obo:RO_0001025 rdf:resource="http://purl.obolibrary.org/obo/GAZ_00007183"/>
        <obo:IAO_0000115>A bank in the Trobriand Islands.</obo:IAO_0000115>
        <oboInOwl:hasOBONamespace>GAZ</oboInOwl:hasOBONamespace>
        <oboInOwl:id>GAZ:00118311</oboInOwl:id>
        <rdfs:label>Rothwell Bank</rdfs:label>
    </owl:NamedIndividual>
    


    <!-- http://purl.obolibrary.org/obo/GAZ_00118312 -->

    <owl:NamedIndividual rdf:about="http://purl.obolibrary.org/obo/GAZ_00118312">
        <obo:RO_0001025 rdf:resource="http://purl.obolibrary.org/obo/GAZ_00007183"/>
        <obo:IAO_0000115>One of the Trobriand Islands.</obo:IAO_0000115>
        <oboInOwl:hasOBONamespace>GAZ</oboInOwl:hasOBONamespace>
        <oboInOwl:id>GAZ:00118312</oboInOwl:id>
        <rdfs:label>Kuyua Island</rdfs:label>
    </owl:NamedIndividual>
    


    <!-- http://purl.obolibrary.org/obo/GAZ_00118313 -->

    <owl:NamedIndividual rdf:about="http://purl.obolibrary.org/obo/GAZ_00118313">
        <obo:RO_0001025 rdf:resource="http://purl.obolibrary.org/obo/GAZ_00007183"/>
        <obo:IAO_0000115>One of the Trobriand Islands.</obo:IAO_0000115>
        <oboInOwl:hasOBONamespace>GAZ</oboInOwl:hasOBONamespace>
        <oboInOwl:id>GAZ:00118313</oboInOwl:id>
        <rdfs:label>Buriwadi Island</rdfs:label>
    </owl:NamedIndividual>
    


    <!-- http://purl.obolibrary.org/obo/GAZ_00118314 -->

    <owl:NamedIndividual rdf:about="http://purl.obolibrary.org/obo/GAZ_00118314">
        <obo:RO_0001025 rdf:resource="http://purl.obolibrary.org/obo/GAZ_00007183"/>
        <obo:IAO_0000115>One of the Trobriand Islands.</obo:IAO_0000115>
        <oboInOwl:hasOBONamespace>GAZ</oboInOwl:hasOBONamespace>
        <oboInOwl:id>GAZ:00118314</oboInOwl:id>
        <rdfs:label>Yaona Island</rdfs:label>
    </owl:NamedIndividual>
    


    <!-- http://purl.obolibrary.org/obo/GAZ_00118315 -->

    <owl:NamedIndividual rdf:about="http://purl.obolibrary.org/obo/GAZ_00118315">
        <obo:RO_0001025 rdf:resource="http://purl.obolibrary.org/obo/GAZ_00007183"/>
        <obo:IAO_0000115>One of the Trobriand Islands.</obo:IAO_0000115>
        <oboInOwl:hasOBONamespace>GAZ</oboInOwl:hasOBONamespace>
        <oboInOwl:id>GAZ:00118315</oboInOwl:id>
        <rdfs:label>Matuga Island</rdfs:label>
    </owl:NamedIndividual>
    


    <!-- http://purl.obolibrary.org/obo/GAZ_00118316 -->

    <owl:NamedIndividual rdf:about="http://purl.obolibrary.org/obo/GAZ_00118316">
        <obo:RO_0001025 rdf:resource="http://purl.obolibrary.org/obo/GAZ_00007183"/>
        <obo:IAO_0000115>One of the Trobriand Islands.</obo:IAO_0000115>
        <oboInOwl:hasOBONamespace>GAZ</oboInOwl:hasOBONamespace>
        <oboInOwl:id>GAZ:00118316</oboInOwl:id>
        <rdfs:label>Nakuana Island</rdfs:label>
    </owl:NamedIndividual>
    


    <!-- http://purl.obolibrary.org/obo/GAZ_00118317 -->

    <owl:NamedIndividual rdf:about="http://purl.obolibrary.org/obo/GAZ_00118317">
        <obo:RO_0001025 rdf:resource="http://purl.obolibrary.org/obo/GAZ_00007183"/>
        <obo:IAO_0000115>One of the Trobriand Islands.</obo:IAO_0000115>
        <oboInOwl:hasOBONamespace>GAZ</oboInOwl:hasOBONamespace>
        <oboInOwl:id>GAZ:00118317</oboInOwl:id>
        <rdfs:label>Boingi Island</rdfs:label>
    </owl:NamedIndividual>
    


    <!-- http://purl.obolibrary.org/obo/GAZ_00118318 -->

    <owl:NamedIndividual rdf:about="http://purl.obolibrary.org/obo/GAZ_00118318">
        <obo:RO_0001025 rdf:resource="http://purl.obolibrary.org/obo/GAZ_00007183"/>
        <obo:IAO_0000115>One of the Trobriand Islands.</obo:IAO_0000115>
        <oboInOwl:hasOBONamespace>GAZ</oboInOwl:hasOBONamespace>
        <oboInOwl:id>GAZ:00118318</oboInOwl:id>
        <rdfs:label>Mu-ua Island</rdfs:label>
    </owl:NamedIndividual>
    


    <!-- http://purl.obolibrary.org/obo/GAZ_00118319 -->

    <owl:NamedIndividual rdf:about="http://purl.obolibrary.org/obo/GAZ_00118319">
        <obo:RO_0001025 rdf:resource="http://purl.obolibrary.org/obo/GAZ_00007183"/>
        <obo:IAO_0000115>One of the Trobriand Islands.</obo:IAO_0000115>
        <oboInOwl:hasOBONamespace>GAZ</oboInOwl:hasOBONamespace>
        <oboInOwl:id>GAZ:00118319</oboInOwl:id>
        <rdfs:label>Iaga Island</rdfs:label>
    </owl:NamedIndividual>
    


    <!-- http://purl.obolibrary.org/obo/GAZ_00118320 -->

    <owl:NamedIndividual rdf:about="http://purl.obolibrary.org/obo/GAZ_00118320">
        <rdf:type rdf:resource="http://purl.obolibrary.org/obo/ENVO_00000220"/>
        <obo:RO_0001025 rdf:resource="http://purl.obolibrary.org/obo/GAZ_00118284"/>
        <obo:IAO_0000115>An island group in the Fly River.</obo:IAO_0000115>
        <oboInOwl:hasOBONamespace>GAZ</oboInOwl:hasOBONamespace>
        <oboInOwl:id>GAZ:00118320</oboInOwl:id>
        <rdfs:label>D&apos;Albertis Fairfax Group</rdfs:label>
    </owl:NamedIndividual>
    


    <!-- http://purl.obolibrary.org/obo/GAZ_00118321 -->

    <owl:NamedIndividual rdf:about="http://purl.obolibrary.org/obo/GAZ_00118321">
        <obo:RO_0001025 rdf:resource="http://purl.obolibrary.org/obo/GAZ_00118284"/>
        <obo:IAO_0000115>An island in the Fly River.</obo:IAO_0000115>
        <oboInOwl:hasOBONamespace>GAZ</oboInOwl:hasOBONamespace>
        <oboInOwl:id>GAZ:00118321</oboInOwl:id>
        <rdfs:label>Tidal Island</rdfs:label>
    </owl:NamedIndividual>
    


    <!-- http://purl.obolibrary.org/obo/GAZ_00118322 -->

    <owl:NamedIndividual rdf:about="http://purl.obolibrary.org/obo/GAZ_00118322">
        <obo:RO_0001025 rdf:resource="http://purl.obolibrary.org/obo/GAZ_00118284"/>
        <obo:IAO_0000115>An island in the Fly River.</obo:IAO_0000115>
        <oboInOwl:hasOBONamespace>GAZ</oboInOwl:hasOBONamespace>
        <oboInOwl:id>GAZ:00118322</oboInOwl:id>
        <rdfs:label>Alligator Island</rdfs:label>
    </owl:NamedIndividual>
    


    <!-- http://purl.obolibrary.org/obo/GAZ_00118323 -->

    <owl:NamedIndividual rdf:about="http://purl.obolibrary.org/obo/GAZ_00118323">
        <obo:RO_0001025 rdf:resource="http://purl.obolibrary.org/obo/GAZ_00007183"/>
        <obo:IAO_0000115>One of the Trobriand Islands.</obo:IAO_0000115>
        <oboInOwl:hasOBONamespace>GAZ</oboInOwl:hasOBONamespace>
        <oboInOwl:id>GAZ:00118323</oboInOwl:id>
        <rdfs:label>Giwagiwa Island</rdfs:label>
    </owl:NamedIndividual>
    


    <!-- http://purl.obolibrary.org/obo/GAZ_00118324 -->

    <owl:NamedIndividual rdf:about="http://purl.obolibrary.org/obo/GAZ_00118324">
        <obo:RO_0001025 rdf:resource="http://purl.obolibrary.org/obo/GAZ_00118320"/>
        <obo:IAO_0000115>An island in the Fly River.</obo:IAO_0000115>
        <oboInOwl:hasOBONamespace>GAZ</oboInOwl:hasOBONamespace>
        <oboInOwl:id>GAZ:00118324</oboInOwl:id>
        <rdfs:label>D&apos;Albertis Island</rdfs:label>
    </owl:NamedIndividual>
    


    <!-- http://purl.obolibrary.org/obo/GAZ_00118325 -->

    <owl:NamedIndividual rdf:about="http://purl.obolibrary.org/obo/GAZ_00118325">
        <obo:RO_0001025 rdf:resource="http://purl.obolibrary.org/obo/GAZ_00118284"/>
        <obo:IAO_0000115>An island in the Fly River.</obo:IAO_0000115>
        <oboInOwl:hasOBONamespace>GAZ</oboInOwl:hasOBONamespace>
        <oboInOwl:id>GAZ:00118325</oboInOwl:id>
        <rdfs:label>Sturt Island</rdfs:label>
    </owl:NamedIndividual>
    


    <!-- http://purl.obolibrary.org/obo/GAZ_00118326 -->

    <owl:NamedIndividual rdf:about="http://purl.obolibrary.org/obo/GAZ_00118326">
        <obo:RO_0001025 rdf:resource="http://purl.obolibrary.org/obo/GAZ_00007183"/>
        <obo:IAO_0000115>One of the Trobriand Islands.</obo:IAO_0000115>
        <oboInOwl:hasOBONamespace>GAZ</oboInOwl:hasOBONamespace>
        <oboInOwl:id>GAZ:00118326</oboInOwl:id>
        <rdfs:label>Nanauli Island</rdfs:label>
    </owl:NamedIndividual>
    


    <!-- http://purl.obolibrary.org/obo/GAZ_00118327 -->

    <owl:NamedIndividual rdf:about="http://purl.obolibrary.org/obo/GAZ_00118327">
        <obo:RO_0001025 rdf:resource="http://purl.obolibrary.org/obo/GAZ_00007183"/>
        <obo:IAO_0000115>One of the Trobriand Islands.</obo:IAO_0000115>
        <oboInOwl:hasOBONamespace>GAZ</oboInOwl:hasOBONamespace>
        <oboInOwl:id>GAZ:00118327</oboInOwl:id>
        <rdfs:label>Wadana Island</rdfs:label>
    </owl:NamedIndividual>
    


    <!-- http://purl.obolibrary.org/obo/GAZ_00118328 -->

    <owl:NamedIndividual rdf:about="http://purl.obolibrary.org/obo/GAZ_00118328">
        <rdf:type rdf:resource="http://purl.obolibrary.org/obo/ENVO_00000220"/>
        <obo:RO_0001025 rdf:resource="http://purl.obolibrary.org/obo/GAZ_00007181"/>
        <obo:IAO_0000115>A small island group in the D&apos;Entrecasteaux Islands, between Goodenough Island and Ferguson Island.</obo:IAO_0000115>
        <oboInOwl:hasOBONamespace>GAZ</oboInOwl:hasOBONamespace>
        <oboInOwl:id>GAZ:00118328</oboInOwl:id>
        <rdfs:label>Barrier Islands</rdfs:label>
    </owl:NamedIndividual>
    


    <!-- http://purl.obolibrary.org/obo/GAZ_00118329 -->

    <owl:NamedIndividual rdf:about="http://purl.obolibrary.org/obo/GAZ_00118329">
        <obo:RO_0001025 rdf:resource="http://purl.obolibrary.org/obo/GAZ_00007181"/>
        <obo:IAO_0000115>An island off the N coast of Goodenough Island.</obo:IAO_0000115>
        <oboInOwl:hasOBONamespace>GAZ</oboInOwl:hasOBONamespace>
        <oboInOwl:id>GAZ:00118329</oboInOwl:id>
        <rdfs:label>Naame Island</rdfs:label>
    </owl:NamedIndividual>
    


    <!-- http://purl.obolibrary.org/obo/GAZ_00118330 -->

    <owl:NamedIndividual rdf:about="http://purl.obolibrary.org/obo/GAZ_00118330">
        <obo:RO_0001025 rdf:resource="http://purl.obolibrary.org/obo/GAZ_00007181"/>
        <obo:IAO_0000115>One of the D&apos;Entrecasteaux Islands.</obo:IAO_0000115>
        <oboInOwl:hasOBONamespace>GAZ</oboInOwl:hasOBONamespace>
        <oboInOwl:id>GAZ:00118330</oboInOwl:id>
        <rdfs:label>Kwailau Island</rdfs:label>
    </owl:NamedIndividual>
    


    <!-- http://purl.obolibrary.org/obo/GAZ_00118331 -->

    <owl:NamedIndividual rdf:about="http://purl.obolibrary.org/obo/GAZ_00118331">
        <obo:RO_0001025 rdf:resource="http://purl.obolibrary.org/obo/GAZ_00007181"/>
        <obo:IAO_0000115>One of the D&apos;Entrecasteaux Islands, N of Ferguson Island.</obo:IAO_0000115>
        <oboInOwl:hasOBONamespace>GAZ</oboInOwl:hasOBONamespace>
        <oboInOwl:id>GAZ:00118331</oboInOwl:id>
        <rdfs:label>Sunday Island</rdfs:label>
    </owl:NamedIndividual>
    


    <!-- http://purl.obolibrary.org/obo/GAZ_00118332 -->

    <owl:NamedIndividual rdf:about="http://purl.obolibrary.org/obo/GAZ_00118332">
        <obo:RO_0001025 rdf:resource="http://purl.obolibrary.org/obo/GAZ_00007181"/>
        <obo:IAO_0000115>One of the D&apos;Entrecasteaux Islands.</obo:IAO_0000115>
        <oboInOwl:hasOBONamespace>GAZ</oboInOwl:hasOBONamespace>
        <oboInOwl:id>GAZ:00118332</oboInOwl:id>
        <rdfs:label>Gumatabu Island</rdfs:label>
    </owl:NamedIndividual>
    


    <!-- http://purl.obolibrary.org/obo/GAZ_00118333 -->

    <owl:NamedIndividual rdf:about="http://purl.obolibrary.org/obo/GAZ_00118333">
        <obo:RO_0001025 rdf:resource="http://purl.obolibrary.org/obo/GAZ_00051595"/>
        <obo:IAO_0000115>One of the Amphlett Islands.</obo:IAO_0000115>
        <oboInOwl:hasOBONamespace>GAZ</oboInOwl:hasOBONamespace>
        <oboInOwl:id>GAZ:00118333</oboInOwl:id>
        <rdfs:label>Wagabu Island</rdfs:label>
    </owl:NamedIndividual>
    


    <!-- http://purl.obolibrary.org/obo/GAZ_00118334 -->

    <owl:NamedIndividual rdf:about="http://purl.obolibrary.org/obo/GAZ_00118334">
        <obo:RO_0001025 rdf:resource="http://purl.obolibrary.org/obo/GAZ_00051595"/>
        <obo:IAO_0000115>One of the Amphlett Islands.</obo:IAO_0000115>
        <oboInOwl:hasOBONamespace>GAZ</oboInOwl:hasOBONamespace>
        <oboInOwl:id>GAZ:00118334</oboInOwl:id>
        <rdfs:label>Wata Island</rdfs:label>
    </owl:NamedIndividual>
    


    <!-- http://purl.obolibrary.org/obo/GAZ_00118335 -->

    <owl:NamedIndividual rdf:about="http://purl.obolibrary.org/obo/GAZ_00118335">
        <obo:RO_0001025 rdf:resource="http://purl.obolibrary.org/obo/GAZ_00051595"/>
        <obo:IAO_0000115>One of the Amphlett Islands.</obo:IAO_0000115>
        <oboInOwl:hasOBONamespace>GAZ</oboInOwl:hasOBONamespace>
        <oboInOwl:id>GAZ:00118335</oboInOwl:id>
        <rdfs:label>Tuboa Island</rdfs:label>
    </owl:NamedIndividual>
    


    <!-- http://purl.obolibrary.org/obo/GAZ_00118336 -->

    <owl:NamedIndividual rdf:about="http://purl.obolibrary.org/obo/GAZ_00118336">
        <obo:RO_0001025 rdf:resource="http://purl.obolibrary.org/obo/GAZ_00051595"/>
        <obo:IAO_0000115>One of the Amphlett Islands.</obo:IAO_0000115>
        <oboInOwl:hasOBONamespace>GAZ</oboInOwl:hasOBONamespace>
        <oboInOwl:id>GAZ:00118336</oboInOwl:id>
        <rdfs:label>Noapoi Island</rdfs:label>
    </owl:NamedIndividual>
    


    <!-- http://purl.obolibrary.org/obo/GAZ_00118337 -->

    <owl:NamedIndividual rdf:about="http://purl.obolibrary.org/obo/GAZ_00118337">
        <obo:RO_0001025 rdf:resource="http://purl.obolibrary.org/obo/GAZ_00051595"/>
        <obo:IAO_0000115>One of the Amphlett Islands.</obo:IAO_0000115>
        <oboInOwl:hasOBONamespace>GAZ</oboInOwl:hasOBONamespace>
        <oboInOwl:id>GAZ:00118337</oboInOwl:id>
        <rdfs:label>Urasi Island</rdfs:label>
    </owl:NamedIndividual>
    


    <!-- http://purl.obolibrary.org/obo/GAZ_00118338 -->

    <owl:NamedIndividual rdf:about="http://purl.obolibrary.org/obo/GAZ_00118338">
        <obo:RO_0001025 rdf:resource="http://purl.obolibrary.org/obo/GAZ_00051595"/>
        <obo:IAO_0000115>One of the Amphlett Islands.</obo:IAO_0000115>
        <oboInOwl:hasOBONamespace>GAZ</oboInOwl:hasOBONamespace>
        <oboInOwl:id>GAZ:00118338</oboInOwl:id>
        <rdfs:label>Wawiwa Island</rdfs:label>
    </owl:NamedIndividual>
    


    <!-- http://purl.obolibrary.org/obo/GAZ_00118339 -->

    <owl:NamedIndividual rdf:about="http://purl.obolibrary.org/obo/GAZ_00118339">
        <obo:RO_0001025 rdf:resource="http://purl.obolibrary.org/obo/GAZ_00051595"/>
        <obo:IAO_0000115>One of the Amphlett Islands.</obo:IAO_0000115>
        <oboInOwl:hasOBONamespace>GAZ</oboInOwl:hasOBONamespace>
        <oboInOwl:id>GAZ:00118339</oboInOwl:id>
        <rdfs:label>Apuo Island</rdfs:label>
    </owl:NamedIndividual>
    


    <!-- http://purl.obolibrary.org/obo/GAZ_00118340 -->

    <owl:NamedIndividual rdf:about="http://purl.obolibrary.org/obo/GAZ_00118340">
        <obo:RO_0001025 rdf:resource="http://purl.obolibrary.org/obo/GAZ_00051595"/>
        <obo:IAO_0000115>One of the Amphlett Islands.</obo:IAO_0000115>
        <oboInOwl:hasOBONamespace>GAZ</oboInOwl:hasOBONamespace>
        <oboInOwl:id>GAZ:00118340</oboInOwl:id>
        <rdfs:label>Toiyana Island</rdfs:label>
    </owl:NamedIndividual>
    


    <!-- http://purl.obolibrary.org/obo/GAZ_00118341 -->

    <owl:NamedIndividual rdf:about="http://purl.obolibrary.org/obo/GAZ_00118341">
        <obo:RO_0001025 rdf:resource="http://purl.obolibrary.org/obo/GAZ_00051595"/>
        <obo:IAO_0000115>One of the Amphlett Islands.</obo:IAO_0000115>
        <oboInOwl:hasOBONamespace>GAZ</oboInOwl:hasOBONamespace>
        <oboInOwl:id>GAZ:00118341</oboInOwl:id>
        <rdfs:label>Wamea Island</rdfs:label>
    </owl:NamedIndividual>
    


    <!-- http://purl.obolibrary.org/obo/GAZ_00118342 -->

    <owl:NamedIndividual rdf:about="http://purl.obolibrary.org/obo/GAZ_00118342">
        <obo:RO_0001025 rdf:resource="http://purl.obolibrary.org/obo/GAZ_00051595"/>
        <obo:IAO_0000115>One of the Amphlett Islands.</obo:IAO_0000115>
        <oboInOwl:hasOBONamespace>GAZ</oboInOwl:hasOBONamespace>
        <oboInOwl:id>GAZ:00118342</oboInOwl:id>
        <rdfs:label>Piatana Island</rdfs:label>
    </owl:NamedIndividual>
    


    <!-- http://purl.obolibrary.org/obo/GAZ_00118343 -->

    <owl:NamedIndividual rdf:about="http://purl.obolibrary.org/obo/GAZ_00118343">
        <obo:RO_0001025 rdf:resource="http://purl.obolibrary.org/obo/GAZ_00051595"/>
        <obo:IAO_0000115>One of the Amphlett Islands.</obo:IAO_0000115>
        <oboInOwl:hasOBONamespace>GAZ</oboInOwl:hasOBONamespace>
        <oboInOwl:id>GAZ:00118343</oboInOwl:id>
        <rdfs:label>Kabona Island</rdfs:label>
    </owl:NamedIndividual>
    


    <!-- http://purl.obolibrary.org/obo/GAZ_00118344 -->

    <owl:NamedIndividual rdf:about="http://purl.obolibrary.org/obo/GAZ_00118344">
        <obo:RO_0001025 rdf:resource="http://purl.obolibrary.org/obo/GAZ_00051595"/>
        <obo:IAO_0000115>One of the Amphlett Islands.</obo:IAO_0000115>
        <oboInOwl:hasOBONamespace>GAZ</oboInOwl:hasOBONamespace>
        <oboInOwl:id>GAZ:00118344</oboInOwl:id>
        <rdfs:label>Watota Island</rdfs:label>
    </owl:NamedIndividual>
    


    <!-- http://purl.obolibrary.org/obo/GAZ_00118345 -->

    <owl:NamedIndividual rdf:about="http://purl.obolibrary.org/obo/GAZ_00118345">
        <obo:RO_0001025 rdf:resource="http://purl.obolibrary.org/obo/GAZ_00051595"/>
        <obo:IAO_0000115>One of the Amphlett Islands.</obo:IAO_0000115>
        <oboInOwl:hasOBONamespace>GAZ</oboInOwl:hasOBONamespace>
        <oboInOwl:id>GAZ:00118345</oboInOwl:id>
        <rdfs:label>Yabwaia Island</rdfs:label>
    </owl:NamedIndividual>
    


    <!-- http://purl.obolibrary.org/obo/GAZ_00118346 -->

    <owl:NamedIndividual rdf:about="http://purl.obolibrary.org/obo/GAZ_00118346">
        <obo:RO_0001025 rdf:resource="http://purl.obolibrary.org/obo/GAZ_00051595"/>
        <obo:IAO_0000115>One of the Amphlett Islands.</obo:IAO_0000115>
        <oboInOwl:hasOBONamespace>GAZ</oboInOwl:hasOBONamespace>
        <oboInOwl:id>GAZ:00118346</oboInOwl:id>
        <rdfs:label>Wawasi Island</rdfs:label>
    </owl:NamedIndividual>
    


    <!-- http://purl.obolibrary.org/obo/GAZ_00118347 -->

    <owl:NamedIndividual rdf:about="http://purl.obolibrary.org/obo/GAZ_00118347">
        <obo:RO_0001025 rdf:resource="http://purl.obolibrary.org/obo/GAZ_00051595"/>
        <obo:IAO_0000115>One of the Amphlett Islands.</obo:IAO_0000115>
        <oboInOwl:hasOBONamespace>GAZ</oboInOwl:hasOBONamespace>
        <oboInOwl:id>GAZ:00118347</oboInOwl:id>
        <rdfs:label>Chalata Island</rdfs:label>
    </owl:NamedIndividual>
    


    <!-- http://purl.obolibrary.org/obo/GAZ_00118348 -->

    <owl:NamedIndividual rdf:about="http://purl.obolibrary.org/obo/GAZ_00118348">
        <obo:RO_0001025 rdf:resource="http://purl.obolibrary.org/obo/GAZ_00051595"/>
        <obo:IAO_0000115>One of the Amphlett Islands.</obo:IAO_0000115>
        <oboInOwl:hasOBONamespace>GAZ</oboInOwl:hasOBONamespace>
        <oboInOwl:id>GAZ:00118348</oboInOwl:id>
        <rdfs:label>Belobeloia Island</rdfs:label>
    </owl:NamedIndividual>
    


    <!-- http://purl.obolibrary.org/obo/GAZ_00118349 -->

    <owl:NamedIndividual rdf:about="http://purl.obolibrary.org/obo/GAZ_00118349">
        <obo:RO_0001025 rdf:resource="http://purl.obolibrary.org/obo/GAZ_00051595"/>
        <obo:IAO_0000115>One of the Amphlett Islands.</obo:IAO_0000115>
        <oboInOwl:hasOBONamespace>GAZ</oboInOwl:hasOBONamespace>
        <oboInOwl:id>GAZ:00118349</oboInOwl:id>
        <rdfs:label>Bialao Island</rdfs:label>
    </owl:NamedIndividual>
    


    <!-- http://purl.obolibrary.org/obo/GAZ_00118350 -->

    <owl:NamedIndividual rdf:about="http://purl.obolibrary.org/obo/GAZ_00118350">
        <obo:RO_0001025 rdf:resource="http://purl.obolibrary.org/obo/GAZ_00007181"/>
        <obo:IAO_0000115>One of the D&apos;Entrecasteaux Islands, to the SE of Dobu Island.</obo:IAO_0000115>
        <oboInOwl:hasOBONamespace>GAZ</oboInOwl:hasOBONamespace>
        <oboInOwl:id>GAZ:00118350</oboInOwl:id>
        <rdfs:label>Sairere Island</rdfs:label>
    </owl:NamedIndividual>
    


    <!-- http://purl.obolibrary.org/obo/GAZ_00118351 -->

    <owl:NamedIndividual rdf:about="http://purl.obolibrary.org/obo/GAZ_00118351">
        <rdf:type rdf:resource="http://purl.obolibrary.org/obo/ENVO_00000220"/>
        <obo:RO_0001025 rdf:resource="http://purl.obolibrary.org/obo/GAZ_00007181"/>
        <obo:IAO_0000115>An island group in the D&apos;Entrecasteaux Islands, off the NW of Normanby Island.</obo:IAO_0000115>
        <oboInOwl:hasOBONamespace>GAZ</oboInOwl:hasOBONamespace>
        <oboInOwl:id>GAZ:00118351</oboInOwl:id>
        <rdfs:label>Souba-Souba Island</rdfs:label>
    </owl:NamedIndividual>
    


    <!-- http://purl.obolibrary.org/obo/GAZ_00118352 -->

    <owl:NamedIndividual rdf:about="http://purl.obolibrary.org/obo/GAZ_00118352">
        <obo:RO_0001025 rdf:resource="http://purl.obolibrary.org/obo/GAZ_00007181"/>
        <obo:RO_0001025 rdf:resource="http://purl.obolibrary.org/obo/GAZ_00118358"/>
        <obo:IAO_0000115>One of the D&apos;Entrecasteaux Islands, off the SW coast of Ferguson Island.</obo:IAO_0000115>
        <oboInOwl:hasOBONamespace>GAZ</oboInOwl:hasOBONamespace>
        <oboInOwl:id>GAZ:00118352</oboInOwl:id>
        <rdfs:label>Lawa Island</rdfs:label>
    </owl:NamedIndividual>
    


    <!-- http://purl.obolibrary.org/obo/GAZ_00118353 -->

    <owl:NamedIndividual rdf:about="http://purl.obolibrary.org/obo/GAZ_00118353">
        <obo:RO_0001025 rdf:resource="http://purl.obolibrary.org/obo/GAZ_00007181"/>
        <obo:IAO_0000115>One of the D&apos;Entrecasteaux Islands, to the NE of Dobu Island.</obo:IAO_0000115>
        <oboInOwl:hasOBONamespace>GAZ</oboInOwl:hasOBONamespace>
        <oboInOwl:id>GAZ:00118353</oboInOwl:id>
        <rdfs:label>Kwaiope Island</rdfs:label>
    </owl:NamedIndividual>
    


    <!-- http://purl.obolibrary.org/obo/GAZ_00118354 -->

    <owl:NamedIndividual rdf:about="http://purl.obolibrary.org/obo/GAZ_00118354">
        <obo:RO_0001025 rdf:resource="http://purl.obolibrary.org/obo/GAZ_00007181"/>
        <obo:IAO_0000115>One of the D&apos;Entrecasteaux Islands, of the NW of Normanby Island.</obo:IAO_0000115>
        <oboInOwl:hasOBONamespace>GAZ</oboInOwl:hasOBONamespace>
        <oboInOwl:id>GAZ:00118354</oboInOwl:id>
        <rdfs:label>Ubuia Island</rdfs:label>
    </owl:NamedIndividual>
    


    <!-- http://purl.obolibrary.org/obo/GAZ_00118355 -->

    <owl:NamedIndividual rdf:about="http://purl.obolibrary.org/obo/GAZ_00118355">
        <obo:RO_0001025 rdf:resource="http://purl.obolibrary.org/obo/GAZ_00007181"/>
        <obo:IAO_0000115>One of the D&apos;Entrecasteaux Islands, off the NW of Normanby Island.</obo:IAO_0000115>
        <oboInOwl:hasOBONamespace>GAZ</oboInOwl:hasOBONamespace>
        <oboInOwl:id>GAZ:00118355</oboInOwl:id>
        <rdfs:label>Observation Island</rdfs:label>
    </owl:NamedIndividual>
    


    <!-- http://purl.obolibrary.org/obo/GAZ_00118356 -->

    <owl:NamedIndividual rdf:about="http://purl.obolibrary.org/obo/GAZ_00118356">
        <obo:RO_0001025 rdf:resource="http://purl.obolibrary.org/obo/GAZ_00007181"/>
        <obo:RO_0001025 rdf:resource="http://purl.obolibrary.org/obo/GAZ_00118357"/>
        <obo:IAO_0000115>One of the D&apos;Entrecasteaux Islands, off the SE coast of Goodenough Island.</obo:IAO_0000115>
        <oboInOwl:hasOBONamespace>GAZ</oboInOwl:hasOBONamespace>
        <oboInOwl:id>GAZ:00118356</oboInOwl:id>
        <rdfs:label>Wagipa Island</rdfs:label>
    </owl:NamedIndividual>
    


    <!-- http://purl.obolibrary.org/obo/GAZ_00118357 -->

    <owl:NamedIndividual rdf:about="http://purl.obolibrary.org/obo/GAZ_00118357">
        <obo:RO_0001025 rdf:resource="http://purl.obolibrary.org/obo/GAZ_00051599"/>
        <obo:IAO_0000115>A straight between Goodenough and Ferguson Islands.</obo:IAO_0000115>
        <oboInOwl:hasOBONamespace>GAZ</oboInOwl:hasOBONamespace>
        <oboInOwl:id>GAZ:00118357</oboInOwl:id>
        <rdfs:label>Moresby Strait</rdfs:label>
    </owl:NamedIndividual>
    


    <!-- http://purl.obolibrary.org/obo/GAZ_00118358 -->

    <owl:NamedIndividual rdf:about="http://purl.obolibrary.org/obo/GAZ_00118358">
        <obo:RO_0001025 rdf:resource="http://purl.obolibrary.org/obo/GAZ_00051599"/>
        <obo:IAO_0000115>A bay at the SW of Ferguson Island.</obo:IAO_0000115>
        <oboInOwl:hasOBONamespace>GAZ</oboInOwl:hasOBONamespace>
        <oboInOwl:id>GAZ:00118358</oboInOwl:id>
        <rdfs:label>Seymour Bay</rdfs:label>
    </owl:NamedIndividual>
    


    <!-- http://purl.obolibrary.org/obo/GAZ_00118359 -->

    <owl:NamedIndividual rdf:about="http://purl.obolibrary.org/obo/GAZ_00118359">
        <obo:RO_0001025 rdf:resource="http://purl.obolibrary.org/obo/GAZ_00007181"/>
        <obo:IAO_0000115>One of the D&apos;Entrecasteaux Islands, to the NE of Normanby Island.</obo:IAO_0000115>
        <oboInOwl:hasOBONamespace>GAZ</oboInOwl:hasOBONamespace>
        <oboInOwl:id>GAZ:00118359</oboInOwl:id>
        <rdfs:label>Duchess Island</rdfs:label>
    </owl:NamedIndividual>
    


    <!-- http://purl.obolibrary.org/obo/GAZ_00118360 -->

    <owl:NamedIndividual rdf:about="http://purl.obolibrary.org/obo/GAZ_00118360">
        <obo:RO_0001025 rdf:resource="http://purl.obolibrary.org/obo/GAZ_00007181"/>
        <obo:IAO_0000115>One of the D&apos;Entrecasteaux Islands, to the NE of Dobu Island.</obo:IAO_0000115>
        <oboInOwl:hasOBONamespace>GAZ</oboInOwl:hasOBONamespace>
        <oboInOwl:id>GAZ:00118360</oboInOwl:id>
        <rdfs:label>Nekumara Island</rdfs:label>
    </owl:NamedIndividual>
    


    <!-- http://purl.obolibrary.org/obo/GAZ_00118361 -->

    <owl:NamedIndividual rdf:about="http://purl.obolibrary.org/obo/GAZ_00118361">
        <obo:RO_0001025 rdf:resource="http://purl.obolibrary.org/obo/GAZ_00007181"/>
        <obo:RO_0001025 rdf:resource="http://purl.obolibrary.org/obo/GAZ_00118362"/>
        <obo:IAO_0000115>One of the D&apos;Entrecasteaux Islands.</obo:IAO_0000115>
        <oboInOwl:hasOBONamespace>GAZ</oboInOwl:hasOBONamespace>
        <oboInOwl:id>GAZ:00118361</oboInOwl:id>
        <rdfs:label>Nedakolana Island</rdfs:label>
    </owl:NamedIndividual>
    


    <!-- http://purl.obolibrary.org/obo/GAZ_00118362 -->

    <owl:NamedIndividual rdf:about="http://purl.obolibrary.org/obo/GAZ_00118362">
        <obo:RO_0001025 rdf:resource="http://purl.obolibrary.org/obo/GAZ_00051599"/>
        <obo:IAO_0000115>A bay on the N of Normanby Island.</obo:IAO_0000115>
        <oboInOwl:hasOBONamespace>GAZ</oboInOwl:hasOBONamespace>
        <oboInOwl:id>GAZ:00118362</oboInOwl:id>
        <rdfs:label>Awaiara Bay</rdfs:label>
    </owl:NamedIndividual>
    


    <!-- http://purl.obolibrary.org/obo/GAZ_00118363 -->

    <owl:NamedIndividual rdf:about="http://purl.obolibrary.org/obo/GAZ_00118363">
        <obo:RO_0001025 rdf:resource="http://purl.obolibrary.org/obo/GAZ_00051740"/>
        <oboInOwl:hasOBONamespace>GAZ</oboInOwl:hasOBONamespace>
        <oboInOwl:id>GAZ:00118363</oboInOwl:id>
        <rdfs:label>Pinipel Atoll</rdfs:label>
    </owl:NamedIndividual>
    


    <!-- http://purl.obolibrary.org/obo/GAZ_00118364 -->

    <owl:NamedIndividual rdf:about="http://purl.obolibrary.org/obo/GAZ_00118364">
        <obo:RO_0001025 rdf:resource="http://purl.obolibrary.org/obo/GAZ_00118363"/>
        <obo:IAO_0000115>A small island on the Pinipel Atoll.</obo:IAO_0000115>
        <oboInOwl:hasOBONamespace>GAZ</oboInOwl:hasOBONamespace>
        <oboInOwl:id>GAZ:00118364</oboInOwl:id>
        <rdfs:label>Sentinel Island</rdfs:label>
    </owl:NamedIndividual>
    


    <!-- http://purl.obolibrary.org/obo/GAZ_00118365 -->

    <owl:NamedIndividual rdf:about="http://purl.obolibrary.org/obo/GAZ_00118365">
        <obo:RO_0001025 rdf:resource="http://purl.obolibrary.org/obo/GAZ_00118363"/>
        <obo:IAO_0000115>A small island on the Pinipel Atoll.</obo:IAO_0000115>
        <oboInOwl:hasOBONamespace>GAZ</oboInOwl:hasOBONamespace>
        <oboInOwl:id>GAZ:00118365</oboInOwl:id>
        <rdfs:label>Sau Island</rdfs:label>
    </owl:NamedIndividual>
    


    <!-- http://purl.obolibrary.org/obo/GAZ_00118366 -->

    <owl:NamedIndividual rdf:about="http://purl.obolibrary.org/obo/GAZ_00118366">
        <obo:RO_0001025 rdf:resource="http://purl.obolibrary.org/obo/GAZ_00051740"/>
        <oboInOwl:hasOBONamespace>GAZ</oboInOwl:hasOBONamespace>
        <oboInOwl:id>GAZ:00118366</oboInOwl:id>
        <rdfs:label>Nissan Atoll</rdfs:label>
    </owl:NamedIndividual>
    


    <!-- http://purl.obolibrary.org/obo/GAZ_00118367 -->

    <owl:NamedIndividual rdf:about="http://purl.obolibrary.org/obo/GAZ_00118367">
        <obo:RO_0001025 rdf:resource="http://purl.obolibrary.org/obo/GAZ_00118366"/>
        <obo:IAO_0000115>A small island on the Nissan Atoll.</obo:IAO_0000115>
        <oboInOwl:hasOBONamespace>GAZ</oboInOwl:hasOBONamespace>
        <oboInOwl:id>GAZ:00118367</oboInOwl:id>
        <rdfs:label>Biot Island</rdfs:label>
    </owl:NamedIndividual>
    


    <!-- http://purl.obolibrary.org/obo/GAZ_00118368 -->

    <owl:NamedIndividual rdf:about="http://purl.obolibrary.org/obo/GAZ_00118368">
        <obo:RO_0001025 rdf:resource="http://purl.obolibrary.org/obo/GAZ_00118366"/>
        <obo:IAO_0000115>An island in the lagoon of Nissan Atoll.</obo:IAO_0000115>
        <oboInOwl:hasOBONamespace>GAZ</oboInOwl:hasOBONamespace>
        <oboInOwl:id>GAZ:00118368</oboInOwl:id>
        <rdfs:label>Hon Island</rdfs:label>
    </owl:NamedIndividual>
    


    <!-- http://purl.obolibrary.org/obo/GAZ_00146248 -->

    <owl:NamedIndividual rdf:about="http://purl.obolibrary.org/obo/GAZ_00146248">
        <obo:IAO_0000115>A 400 km wide region on the south shore of New Guinea. Some of New Guinea&apos;s largest rivers, such as the Fly River, Turama River, Kikori River and Purari River, flow into the gulf, making it a large delta.</obo:IAO_0000115>
        <oboInOwl:hasOBONamespace>GAZ</oboInOwl:hasOBONamespace>
        <oboInOwl:id>GAZ:00146248</oboInOwl:id>
        <rdfs:label>Gulf of Papua</rdfs:label>
    </owl:NamedIndividual>
    


    <!-- http://purl.obolibrary.org/obo/GAZ_00146249 -->

    <owl:NamedIndividual rdf:about="http://purl.obolibrary.org/obo/GAZ_00146249">
        <obo:RO_0001025 rdf:resource="http://purl.obolibrary.org/obo/GAZ_00146248"/>
        <obo:IAO_0000115>A body of water in southeastern Papua New Guinea, south of Port Moresby.</obo:IAO_0000115>
        <oboInOwl:hasOBONamespace>GAZ</oboInOwl:hasOBONamespace>
        <oboInOwl:id>GAZ:00146249</oboInOwl:id>
        <rdfs:label>Bootless Inlet</rdfs:label>
    </owl:NamedIndividual>
    


    <!-- http://purl.obolibrary.org/obo/GAZ_00146834 -->

    <owl:NamedIndividual rdf:about="http://purl.obolibrary.org/obo/GAZ_00146834">
        <obo:RO_0001025 rdf:resource="http://purl.obolibrary.org/obo/GAZ_00005198"/>
        <obo:IAO_0000115>A large body of water off the south coast of Madang Province, Papua New Guinea. It is a part of the Bismarck Sea and stretches from the Cape Iris in the south to the Cape Croisilles to the north.</obo:IAO_0000115>
        <oboInOwl:hasOBONamespace>GAZ</oboInOwl:hasOBONamespace>
        <oboInOwl:id>GAZ:00146834</oboInOwl:id>
        <rdfs:label>Astrolabe Bay</rdfs:label>
    </owl:NamedIndividual>
    


    <!-- http://purl.obolibrary.org/obo/GAZ_00146835 -->

    <owl:NamedIndividual rdf:about="http://purl.obolibrary.org/obo/GAZ_00146835">
        <obo:RO_0001025 rdf:resource="http://purl.obolibrary.org/obo/GAZ_00005184"/>
        <obo:IAO_0000115>A bay on the western side of the island of Bougainville, in Papua New Guinea.</obo:IAO_0000115>
        <oboInOwl:hasOBONamespace>GAZ</oboInOwl:hasOBONamespace>
        <oboInOwl:id>GAZ:00146835</oboInOwl:id>
        <rdfs:label>Empress Augusta Bay</rdfs:label>
    </owl:NamedIndividual>
    


    <!-- http://purl.obolibrary.org/obo/GAZ_00146836 -->

    <owl:NamedIndividual rdf:about="http://purl.obolibrary.org/obo/GAZ_00146836">
        <obo:RO_0001025 rdf:resource="http://purl.obolibrary.org/obo/GAZ_00012662"/>
        <obo:IAO_0000115>A bay in Oro Province, southeastern Papua New Guinea.</obo:IAO_0000115>
        <oboInOwl:hasOBONamespace>GAZ</oboInOwl:hasOBONamespace>
        <oboInOwl:id>GAZ:00146836</oboInOwl:id>
        <rdfs:label>Holnicote Bay</rdfs:label>
    </owl:NamedIndividual>
    


    <!-- http://purl.obolibrary.org/obo/GAZ_00146837 -->

    <owl:NamedIndividual rdf:about="http://purl.obolibrary.org/obo/GAZ_00146837">
        <obo:RO_0001025 rdf:resource="http://purl.obolibrary.org/obo/GAZ_00005192"/>
        <obo:IAO_0000115>A bay in East New Britain Province, southeastern New Britain, Papua New Guinea.</obo:IAO_0000115>
        <oboInOwl:hasOBONamespace>GAZ</oboInOwl:hasOBONamespace>
        <oboInOwl:id>GAZ:00146837</oboInOwl:id>
        <rdfs:label>Jacquinot Bay</rdfs:label>
    </owl:NamedIndividual>
    


    <!-- http://purl.obolibrary.org/obo/GAZ_00146838 -->

    <owl:NamedIndividual rdf:about="http://purl.obolibrary.org/obo/GAZ_00146838">
        <obo:RO_0001025 rdf:resource="http://purl.obolibrary.org/obo/GAZ_00005189"/>
        <obo:RO_0001025 rdf:resource="http://purl.obolibrary.org/obo/GAZ_00253918"/>
        <obo:IAO_0000115>A large bay in West New Britain Province, off the northern coast of New Britain, Papua New Guinea.</obo:IAO_0000115>
        <oboInOwl:hasOBONamespace>GAZ</oboInOwl:hasOBONamespace>
        <oboInOwl:id>GAZ:00146838</oboInOwl:id>
        <rdfs:label>Kimbe Bay</rdfs:label>
    </owl:NamedIndividual>
    


    <!-- http://purl.obolibrary.org/obo/GAZ_00146841 -->

    <owl:NamedIndividual rdf:about="http://purl.obolibrary.org/obo/GAZ_00146841">
        <obo:RO_0001025 rdf:resource="http://purl.obolibrary.org/obo/GAZ_00012662"/>
        <obo:IAO_0000115>A bay in Oro Province of Papua New Guinea.</obo:IAO_0000115>
        <oboInOwl:hasOBONamespace>GAZ</oboInOwl:hasOBONamespace>
        <oboInOwl:id>GAZ:00146841</oboInOwl:id>
        <rdfs:label>Oro Bay</rdfs:label>
    </owl:NamedIndividual>
    


    <!-- http://purl.obolibrary.org/obo/GAZ_00146842 -->

    <owl:NamedIndividual rdf:about="http://purl.obolibrary.org/obo/GAZ_00146842">
        <obo:RO_0001025 rdf:resource="http://purl.obolibrary.org/obo/GAZ_00253585"/>
        <obo:IAO_0000115>A bay within Dyke Ackland Bay, Northern Province of Papua New Guinea.</obo:IAO_0000115>
        <oboInOwl:hasOBONamespace>GAZ</oboInOwl:hasOBONamespace>
        <oboInOwl:id>GAZ:00146842</oboInOwl:id>
        <rdfs:label>Porlock Bay</rdfs:label>
    </owl:NamedIndividual>
    


    <!-- http://purl.obolibrary.org/obo/GAZ_00146843 -->

    <owl:NamedIndividual rdf:about="http://purl.obolibrary.org/obo/GAZ_00146843">
        <obo:RO_0001025 rdf:resource="http://purl.obolibrary.org/obo/GAZ_00051599"/>
        <obo:IAO_0000115>A bay on the north west shore of Milne Bay, Papua New Guinea.</obo:IAO_0000115>
        <oboInOwl:hasOBONamespace>GAZ</oboInOwl:hasOBONamespace>
        <oboInOwl:id>GAZ:00146843</oboInOwl:id>
        <rdfs:label>Swinger Bay</rdfs:label>
    </owl:NamedIndividual>
    


    <!-- http://purl.obolibrary.org/obo/GAZ_00146844 -->

    <owl:NamedIndividual rdf:about="http://purl.obolibrary.org/obo/GAZ_00146844">
        <obo:RO_0001025 rdf:resource="http://purl.obolibrary.org/obo/GAZ_00005192"/>
        <obo:IAO_0000115>A bay in East New Britain Province, southeastern New Britain, Papua New Guinea.</obo:IAO_0000115>
        <oboInOwl:hasOBONamespace>GAZ</oboInOwl:hasOBONamespace>
        <oboInOwl:id>GAZ:00146844</oboInOwl:id>
        <rdfs:label>Waterfall Bay</rdfs:label>
    </owl:NamedIndividual>
    


    <!-- http://purl.obolibrary.org/obo/GAZ_00147123 -->

    <owl:NamedIndividual rdf:about="http://purl.obolibrary.org/obo/GAZ_00147123">
        <rdf:type rdf:resource="http://purl.obolibrary.org/obo/ENVO_00000305"/>
        <obo:RO_0001025 rdf:resource="http://purl.obolibrary.org/obo/GAZ_00012662"/>
        <obo:IAO_0000115>A cape in Papua New Guinea, next to Oro Bay. It is situated in Northern Province, about a mile south of Hariko.</obo:IAO_0000115>
        <oboInOwl:hasOBONamespace>GAZ</oboInOwl:hasOBONamespace>
        <oboInOwl:id>GAZ:00147123</oboInOwl:id>
        <rdfs:label>Cape Sudest</rdfs:label>
    </owl:NamedIndividual>
    


    <!-- http://purl.obolibrary.org/obo/GAZ_00147124 -->

    <owl:NamedIndividual rdf:about="http://purl.obolibrary.org/obo/GAZ_00147124">
        <obo:RO_0001025 rdf:resource="http://purl.obolibrary.org/obo/GAZ_00005182"/>
        <obo:RO_0001025 rdf:resource="http://purl.obolibrary.org/obo/GAZ_00005189"/>
        <obo:IAO_0000115>A headland, in the northwest of the island of New Britain, Papua New Guinea.</obo:IAO_0000115>
        <oboInOwl:hasOBONamespace>GAZ</oboInOwl:hasOBONamespace>
        <oboInOwl:id>GAZ:00147124</oboInOwl:id>
        <rdfs:label>Cape Gloucester</rdfs:label>
    </owl:NamedIndividual>
    


    <!-- http://purl.obolibrary.org/obo/GAZ_00147125 -->

    <owl:NamedIndividual rdf:about="http://purl.obolibrary.org/obo/GAZ_00147125">
        <obo:RO_0001025 rdf:resource="http://purl.obolibrary.org/obo/GAZ_00005188"/>
        <obo:IAO_0000115>The southernmost point on the island of New Ireland, Papua New Guinea.</obo:IAO_0000115>
        <oboInOwl:hasOBONamespace>GAZ</oboInOwl:hasOBONamespace>
        <oboInOwl:id>GAZ:00147125</oboInOwl:id>
        <rdfs:label>Cape Saint George</rdfs:label>
    </owl:NamedIndividual>
    


    <!-- http://purl.obolibrary.org/obo/GAZ_00147126 -->

    <owl:NamedIndividual rdf:about="http://purl.obolibrary.org/obo/GAZ_00147126">
        <rdf:type rdf:resource="http://purl.obolibrary.org/obo/ENVO_00000305"/>
        <obo:RO_0001025 rdf:resource="http://purl.obolibrary.org/obo/GAZ_00005189"/>
        <obo:RO_0001025 rdf:resource="http://purl.obolibrary.org/obo/GAZ_00005191"/>
        <obo:IAO_0000115>A headland in the north-central of the island of New Britain, Papua New Guinea.</obo:IAO_0000115>
        <oboInOwl:hasOBONamespace>GAZ</oboInOwl:hasOBONamespace>
        <oboInOwl:id>GAZ:00147126</oboInOwl:id>
        <rdfs:label>Cape Hollman</rdfs:label>
    </owl:NamedIndividual>
    


    <!-- http://purl.obolibrary.org/obo/GAZ_00147127 -->

    <owl:NamedIndividual rdf:about="http://purl.obolibrary.org/obo/GAZ_00147127">
        <rdf:type rdf:resource="http://purl.obolibrary.org/obo/ENVO_00000305"/>
        <obo:RO_0001025 rdf:resource="http://purl.obolibrary.org/obo/GAZ_00005184"/>
        <obo:IAO_0000115>A headland at the north end of Empress Augusta Bay, along the central part of the southeastern coast of Bougainville, in Papua New Guinea.</obo:IAO_0000115>
        <oboInOwl:hasOBONamespace>GAZ</oboInOwl:hasOBONamespace>
        <oboInOwl:id>GAZ:00147127</oboInOwl:id>
        <rdfs:label>Cape Torokina</rdfs:label>
    </owl:NamedIndividual>
    


    <!-- http://purl.obolibrary.org/obo/GAZ_00250591 -->

    <owl:NamedIndividual rdf:about="http://purl.obolibrary.org/obo/GAZ_00250591">
        <obo:RO_0001025 rdf:resource="http://purl.obolibrary.org/obo/GAZ_00118285"/>
        <obo:IAO_0000115>An island in the Fly River Delta.</obo:IAO_0000115>
        <oboInOwl:hasOBONamespace>GAZ</oboInOwl:hasOBONamespace>
        <oboInOwl:id>GAZ:00250591</oboInOwl:id>
        <rdfs:label>Aibinio Island</rdfs:label>
    </owl:NamedIndividual>
    


    <!-- http://purl.obolibrary.org/obo/GAZ_00250592 -->

    <owl:NamedIndividual rdf:about="http://purl.obolibrary.org/obo/GAZ_00250592">
        <obo:RO_0001025 rdf:resource="http://purl.obolibrary.org/obo/GAZ_00118285"/>
        <obo:IAO_0000115>An island in the Fly River Delta.</obo:IAO_0000115>
        <oboInOwl:hasOBONamespace>GAZ</oboInOwl:hasOBONamespace>
        <oboInOwl:id>GAZ:00250592</oboInOwl:id>
        <rdfs:label>Mibu Island</rdfs:label>
    </owl:NamedIndividual>
    


    <!-- http://purl.obolibrary.org/obo/GAZ_00250593 -->

    <owl:NamedIndividual rdf:about="http://purl.obolibrary.org/obo/GAZ_00250593">
        <obo:RO_0001025 rdf:resource="http://purl.obolibrary.org/obo/GAZ_00118285"/>
        <obo:IAO_0000115>An island in the Fly River Delta.</obo:IAO_0000115>
        <oboInOwl:hasOBONamespace>GAZ</oboInOwl:hasOBONamespace>
        <oboInOwl:id>GAZ:00250593</oboInOwl:id>
        <rdfs:label>Magabu Island</rdfs:label>
    </owl:NamedIndividual>
    


    <!-- http://purl.obolibrary.org/obo/GAZ_00250594 -->

    <owl:NamedIndividual rdf:about="http://purl.obolibrary.org/obo/GAZ_00250594">
        <obo:RO_0001025 rdf:resource="http://purl.obolibrary.org/obo/GAZ_00118285"/>
        <obo:IAO_0000115>An island in the Fly River Delta.</obo:IAO_0000115>
        <oboInOwl:hasOBONamespace>GAZ</oboInOwl:hasOBONamespace>
        <oboInOwl:id>GAZ:00250594</oboInOwl:id>
        <rdfs:label>Invitato Island</rdfs:label>
    </owl:NamedIndividual>
    


    <!-- http://purl.obolibrary.org/obo/GAZ_00250595 -->

    <owl:NamedIndividual rdf:about="http://purl.obolibrary.org/obo/GAZ_00250595">
        <obo:RO_0001025 rdf:resource="http://purl.obolibrary.org/obo/GAZ_00118285"/>
        <obo:IAO_0000115>An island in the Fly River Delta.</obo:IAO_0000115>
        <oboInOwl:hasOBONamespace>GAZ</oboInOwl:hasOBONamespace>
        <oboInOwl:id>GAZ:00250595</oboInOwl:id>
        <rdfs:label>Sisiabu Island</rdfs:label>
    </owl:NamedIndividual>
    


    <!-- http://purl.obolibrary.org/obo/GAZ_00250596 -->

    <owl:NamedIndividual rdf:about="http://purl.obolibrary.org/obo/GAZ_00250596">
        <obo:RO_0001025 rdf:resource="http://purl.obolibrary.org/obo/GAZ_00118285"/>
        <obo:IAO_0000115>An island in the Fly River Delta.</obo:IAO_0000115>
        <oboInOwl:hasOBONamespace>GAZ</oboInOwl:hasOBONamespace>
        <oboInOwl:id>GAZ:00250596</oboInOwl:id>
        <rdfs:label>Nikira Island</rdfs:label>
    </owl:NamedIndividual>
    


    <!-- http://purl.obolibrary.org/obo/GAZ_00250597 -->

    <owl:NamedIndividual rdf:about="http://purl.obolibrary.org/obo/GAZ_00250597">
        <obo:RO_0001025 rdf:resource="http://purl.obolibrary.org/obo/GAZ_00118285"/>
        <obo:IAO_0000115>An island in the Fly River Delta.</obo:IAO_0000115>
        <oboInOwl:hasOBONamespace>GAZ</oboInOwl:hasOBONamespace>
        <oboInOwl:id>GAZ:00250597</oboInOwl:id>
        <rdfs:label>Badu Island</rdfs:label>
    </owl:NamedIndividual>
    


    <!-- http://purl.obolibrary.org/obo/GAZ_00250598 -->

    <owl:NamedIndividual rdf:about="http://purl.obolibrary.org/obo/GAZ_00250598">
        <obo:RO_0001025 rdf:resource="http://purl.obolibrary.org/obo/GAZ_00118285"/>
        <obo:IAO_0000115>An island in the Fly River Delta.</obo:IAO_0000115>
        <oboInOwl:hasOBONamespace>GAZ</oboInOwl:hasOBONamespace>
        <oboInOwl:id>GAZ:00250598</oboInOwl:id>
        <rdfs:label>Baiabe Island</rdfs:label>
    </owl:NamedIndividual>
    


    <!-- http://purl.obolibrary.org/obo/GAZ_00250599 -->

    <owl:NamedIndividual rdf:about="http://purl.obolibrary.org/obo/GAZ_00250599">
        <obo:RO_0001025 rdf:resource="http://purl.obolibrary.org/obo/GAZ_00118285"/>
        <obo:IAO_0000115>An island in the Fly River Delta.</obo:IAO_0000115>
        <oboInOwl:hasOBONamespace>GAZ</oboInOwl:hasOBONamespace>
        <oboInOwl:id>GAZ:00250599</oboInOwl:id>
        <rdfs:label>Moroge Island</rdfs:label>
    </owl:NamedIndividual>
    


    <!-- http://purl.obolibrary.org/obo/GAZ_00250600 -->

    <owl:NamedIndividual rdf:about="http://purl.obolibrary.org/obo/GAZ_00250600">
        <obo:RO_0001025 rdf:resource="http://purl.obolibrary.org/obo/GAZ_00118285"/>
        <obo:IAO_0000115>An island in the Fly River Delta.</obo:IAO_0000115>
        <oboInOwl:hasOBONamespace>GAZ</oboInOwl:hasOBONamespace>
        <oboInOwl:id>GAZ:00250600</oboInOwl:id>
        <rdfs:label>Gebaro Island</rdfs:label>
    </owl:NamedIndividual>
    


    <!-- http://purl.obolibrary.org/obo/GAZ_00250601 -->

    <owl:NamedIndividual rdf:about="http://purl.obolibrary.org/obo/GAZ_00250601">
        <obo:RO_0001025 rdf:resource="http://purl.obolibrary.org/obo/GAZ_00118285"/>
        <obo:IAO_0000115>An island in the Fly River Delta.</obo:IAO_0000115>
        <oboInOwl:hasOBONamespace>GAZ</oboInOwl:hasOBONamespace>
        <oboInOwl:id>GAZ:00250601</oboInOwl:id>
        <rdfs:label>Dawari Island</rdfs:label>
    </owl:NamedIndividual>
    


    <!-- http://purl.obolibrary.org/obo/GAZ_00250602 -->

    <owl:NamedIndividual rdf:about="http://purl.obolibrary.org/obo/GAZ_00250602">
        <obo:RO_0001025 rdf:resource="http://purl.obolibrary.org/obo/GAZ_00118285"/>
        <obo:IAO_0000115>An island in the Fly River Delta.</obo:IAO_0000115>
        <oboInOwl:hasOBONamespace>GAZ</oboInOwl:hasOBONamespace>
        <oboInOwl:id>GAZ:00250602</oboInOwl:id>
        <rdfs:label>Wariura Island</rdfs:label>
    </owl:NamedIndividual>
    


    <!-- http://purl.obolibrary.org/obo/GAZ_00250603 -->

    <owl:NamedIndividual rdf:about="http://purl.obolibrary.org/obo/GAZ_00250603">
        <obo:RO_0001025 rdf:resource="http://purl.obolibrary.org/obo/GAZ_00118285"/>
        <obo:IAO_0000115>An island in the Fly River Delta.</obo:IAO_0000115>
        <oboInOwl:hasOBONamespace>GAZ</oboInOwl:hasOBONamespace>
        <oboInOwl:id>GAZ:00250603</oboInOwl:id>
        <rdfs:label>War Island</rdfs:label>
    </owl:NamedIndividual>
    


    <!-- http://purl.obolibrary.org/obo/GAZ_00250604 -->

    <owl:NamedIndividual rdf:about="http://purl.obolibrary.org/obo/GAZ_00250604">
        <obo:RO_0001025 rdf:resource="http://purl.obolibrary.org/obo/GAZ_00118285"/>
        <obo:IAO_0000115>An island in the Fly River Delta.</obo:IAO_0000115>
        <oboInOwl:hasOBONamespace>GAZ</oboInOwl:hasOBONamespace>
        <oboInOwl:id>GAZ:00250604</oboInOwl:id>
        <rdfs:label>Kesuguruguru Island</rdfs:label>
    </owl:NamedIndividual>
    


    <!-- http://purl.obolibrary.org/obo/GAZ_00250605 -->

    <owl:NamedIndividual rdf:about="http://purl.obolibrary.org/obo/GAZ_00250605">
        <obo:RO_0001025 rdf:resource="http://purl.obolibrary.org/obo/GAZ_00118285"/>
        <obo:IAO_0000115>An island in the Fly River Delta.</obo:IAO_0000115>
        <oboInOwl:hasOBONamespace>GAZ</oboInOwl:hasOBONamespace>
        <oboInOwl:id>GAZ:00250605</oboInOwl:id>
        <rdfs:label>Abaura Island</rdfs:label>
    </owl:NamedIndividual>
    


    <!-- http://purl.obolibrary.org/obo/GAZ_00250606 -->

    <owl:NamedIndividual rdf:about="http://purl.obolibrary.org/obo/GAZ_00250606">
        <obo:RO_0001025 rdf:resource="http://purl.obolibrary.org/obo/GAZ_00118285"/>
        <obo:IAO_0000115>An island in the Fly River Delta.</obo:IAO_0000115>
        <oboInOwl:hasOBONamespace>GAZ</oboInOwl:hasOBONamespace>
        <oboInOwl:id>GAZ:00250606</oboInOwl:id>
        <rdfs:label>Abo Island</rdfs:label>
    </owl:NamedIndividual>
    


    <!-- http://purl.obolibrary.org/obo/GAZ_00250607 -->

    <owl:NamedIndividual rdf:about="http://purl.obolibrary.org/obo/GAZ_00250607">
        <obo:RO_0001025 rdf:resource="http://purl.obolibrary.org/obo/GAZ_00118285"/>
        <obo:IAO_0000115>An island in the Fly River Delta.</obo:IAO_0000115>
        <oboInOwl:hasOBONamespace>GAZ</oboInOwl:hasOBONamespace>
        <oboInOwl:id>GAZ:00250607</oboInOwl:id>
        <rdfs:label>Boromura Island</rdfs:label>
    </owl:NamedIndividual>
    


    <!-- http://purl.obolibrary.org/obo/GAZ_00250608 -->

    <owl:NamedIndividual rdf:about="http://purl.obolibrary.org/obo/GAZ_00250608">
        <obo:RO_0001025 rdf:resource="http://purl.obolibrary.org/obo/GAZ_00118285"/>
        <obo:IAO_0000115>An island in the Fly River Delta.</obo:IAO_0000115>
        <oboInOwl:hasOBONamespace>GAZ</oboInOwl:hasOBONamespace>
        <oboInOwl:id>GAZ:00250608</oboInOwl:id>
        <rdfs:label>Ura Island</rdfs:label>
    </owl:NamedIndividual>
    


    <!-- http://purl.obolibrary.org/obo/GAZ_00250609 -->

    <owl:NamedIndividual rdf:about="http://purl.obolibrary.org/obo/GAZ_00250609">
        <obo:RO_0001025 rdf:resource="http://purl.obolibrary.org/obo/GAZ_00118285"/>
        <obo:IAO_0000115>An island in the Fly River Delta.</obo:IAO_0000115>
        <oboInOwl:hasOBONamespace>GAZ</oboInOwl:hasOBONamespace>
        <oboInOwl:id>GAZ:00250609</oboInOwl:id>
        <rdfs:label>Dogope Island</rdfs:label>
    </owl:NamedIndividual>
    


    <!-- http://purl.obolibrary.org/obo/GAZ_00250610 -->

    <owl:NamedIndividual rdf:about="http://purl.obolibrary.org/obo/GAZ_00250610">
        <obo:RO_0001025 rdf:resource="http://purl.obolibrary.org/obo/GAZ_00118285"/>
        <obo:IAO_0000115>An island in the Fly River Delta.</obo:IAO_0000115>
        <oboInOwl:hasOBONamespace>GAZ</oboInOwl:hasOBONamespace>
        <oboInOwl:id>GAZ:00250610</oboInOwl:id>
        <rdfs:label>Sumogi Island</rdfs:label>
    </owl:NamedIndividual>
    


    <!-- http://purl.obolibrary.org/obo/GAZ_00250611 -->

    <owl:NamedIndividual rdf:about="http://purl.obolibrary.org/obo/GAZ_00250611">
        <obo:RO_0001025 rdf:resource="http://purl.obolibrary.org/obo/GAZ_00118285"/>
        <obo:IAO_0000115>An island in the Fly River Delta.</obo:IAO_0000115>
        <oboInOwl:hasOBONamespace>GAZ</oboInOwl:hasOBONamespace>
        <oboInOwl:id>GAZ:00250611</oboInOwl:id>
        <rdfs:label>Sobowada Island</rdfs:label>
    </owl:NamedIndividual>
    


    <!-- http://purl.obolibrary.org/obo/GAZ_00250612 -->

    <owl:NamedIndividual rdf:about="http://purl.obolibrary.org/obo/GAZ_00250612">
        <obo:RO_0001025 rdf:resource="http://purl.obolibrary.org/obo/GAZ_00118285"/>
        <obo:IAO_0000115>An island in the Fly River Delta.</obo:IAO_0000115>
        <oboInOwl:hasOBONamespace>GAZ</oboInOwl:hasOBONamespace>
        <oboInOwl:id>GAZ:00250612</oboInOwl:id>
        <rdfs:label>Abaurai Island</rdfs:label>
    </owl:NamedIndividual>
    


    <!-- http://purl.obolibrary.org/obo/GAZ_00250613 -->

    <owl:NamedIndividual rdf:about="http://purl.obolibrary.org/obo/GAZ_00250613">
        <obo:RO_0001025 rdf:resource="http://purl.obolibrary.org/obo/GAZ_00118285"/>
        <obo:IAO_0000115>An island in the Fly River Delta.</obo:IAO_0000115>
        <oboInOwl:hasOBONamespace>GAZ</oboInOwl:hasOBONamespace>
        <oboInOwl:id>GAZ:00250613</oboInOwl:id>
        <rdfs:label>Samari Island</rdfs:label>
    </owl:NamedIndividual>
    


    <!-- http://purl.obolibrary.org/obo/GAZ_00250614 -->

    <owl:NamedIndividual rdf:about="http://purl.obolibrary.org/obo/GAZ_00250614">
        <obo:RO_0001025 rdf:resource="http://purl.obolibrary.org/obo/GAZ_00118285"/>
        <obo:IAO_0000115>An island in the Fly River Delta.</obo:IAO_0000115>
        <oboInOwl:hasOBONamespace>GAZ</oboInOwl:hasOBONamespace>
        <oboInOwl:id>GAZ:00250614</oboInOwl:id>
        <rdfs:label>Reginimi Island</rdfs:label>
    </owl:NamedIndividual>
    


    <!-- http://purl.obolibrary.org/obo/GAZ_00250615 -->

    <owl:NamedIndividual rdf:about="http://purl.obolibrary.org/obo/GAZ_00250615">
        <obo:RO_0001025 rdf:resource="http://purl.obolibrary.org/obo/GAZ_00118285"/>
        <obo:IAO_0000115>An island in the Fly River Delta.</obo:IAO_0000115>
        <oboInOwl:hasOBONamespace>GAZ</oboInOwl:hasOBONamespace>
        <oboInOwl:id>GAZ:00250615</oboInOwl:id>
        <rdfs:label>Dibiri Island</rdfs:label>
    </owl:NamedIndividual>
    


    <!-- http://purl.obolibrary.org/obo/GAZ_00250616 -->

    <owl:NamedIndividual rdf:about="http://purl.obolibrary.org/obo/GAZ_00250616">
        <obo:RO_0001025 rdf:resource="http://purl.obolibrary.org/obo/GAZ_00118285"/>
        <obo:IAO_0000115>An island in the Fly River Delta.</obo:IAO_0000115>
        <oboInOwl:hasOBONamespace>GAZ</oboInOwl:hasOBONamespace>
        <oboInOwl:id>GAZ:00250616</oboInOwl:id>
        <rdfs:label>Sobuwabuda Island</rdfs:label>
    </owl:NamedIndividual>
    


    <!-- http://purl.obolibrary.org/obo/GAZ_00250617 -->

    <owl:NamedIndividual rdf:about="http://purl.obolibrary.org/obo/GAZ_00250617">
        <obo:RO_0001025 rdf:resource="http://purl.obolibrary.org/obo/GAZ_00118285"/>
        <obo:IAO_0000115>An island in the Fly River Delta.</obo:IAO_0000115>
        <oboInOwl:hasOBONamespace>GAZ</oboInOwl:hasOBONamespace>
        <oboInOwl:id>GAZ:00250617</oboInOwl:id>
        <rdfs:label>Orope Island</rdfs:label>
    </owl:NamedIndividual>
    


    <!-- http://purl.obolibrary.org/obo/GAZ_00250618 -->

    <owl:NamedIndividual rdf:about="http://purl.obolibrary.org/obo/GAZ_00250618">
        <obo:RO_0001025 rdf:resource="http://purl.obolibrary.org/obo/GAZ_00118285"/>
        <obo:IAO_0000115>An island in the Fly River Delta.</obo:IAO_0000115>
        <oboInOwl:hasOBONamespace>GAZ</oboInOwl:hasOBONamespace>
        <oboInOwl:id>GAZ:00250618</oboInOwl:id>
        <rdfs:label>Aeginimi Islands</rdfs:label>
    </owl:NamedIndividual>
    


    <!-- http://purl.obolibrary.org/obo/GAZ_00250619 -->

    <owl:NamedIndividual rdf:about="http://purl.obolibrary.org/obo/GAZ_00250619">
        <obo:RO_0001025 rdf:resource="http://purl.obolibrary.org/obo/GAZ_00118285"/>
        <obo:IAO_0000115>An island in the Fly River Delta.</obo:IAO_0000115>
        <oboInOwl:hasOBONamespace>GAZ</oboInOwl:hasOBONamespace>
        <oboInOwl:id>GAZ:00250619</oboInOwl:id>
        <rdfs:label>Umuda Island</rdfs:label>
    </owl:NamedIndividual>
    


    <!-- http://purl.obolibrary.org/obo/GAZ_00250620 -->

    <owl:NamedIndividual rdf:about="http://purl.obolibrary.org/obo/GAZ_00250620">
        <obo:RO_0001025 rdf:resource="http://purl.obolibrary.org/obo/GAZ_00118285"/>
        <obo:IAO_0000115>An island in the Fly River Delta.</obo:IAO_0000115>
        <oboInOwl:hasOBONamespace>GAZ</oboInOwl:hasOBONamespace>
        <oboInOwl:id>GAZ:00250620</oboInOwl:id>
        <rdfs:label>Midima Island</rdfs:label>
    </owl:NamedIndividual>
    


    <!-- http://purl.obolibrary.org/obo/GAZ_00250621 -->

    <owl:NamedIndividual rdf:about="http://purl.obolibrary.org/obo/GAZ_00250621">
        <obo:RO_0001025 rdf:resource="http://purl.obolibrary.org/obo/GAZ_00118285"/>
        <obo:IAO_0000115>An island in the Fly River Delta.</obo:IAO_0000115>
        <oboInOwl:hasOBONamespace>GAZ</oboInOwl:hasOBONamespace>
        <oboInOwl:id>GAZ:00250621</oboInOwl:id>
        <rdfs:label>Domori Island</rdfs:label>
    </owl:NamedIndividual>
    


    <!-- http://purl.obolibrary.org/obo/GAZ_00250622 -->

    <owl:NamedIndividual rdf:about="http://purl.obolibrary.org/obo/GAZ_00250622">
        <obo:RO_0001025 rdf:resource="http://purl.obolibrary.org/obo/GAZ_00118285"/>
        <obo:IAO_0000115>An island in the Fly River Delta.</obo:IAO_0000115>
        <oboInOwl:hasOBONamespace>GAZ</oboInOwl:hasOBONamespace>
        <oboInOwl:id>GAZ:00250622</oboInOwl:id>
        <rdfs:label>Dubuwaro Island</rdfs:label>
    </owl:NamedIndividual>
    


    <!-- http://purl.obolibrary.org/obo/GAZ_00250623 -->

    <owl:NamedIndividual rdf:about="http://purl.obolibrary.org/obo/GAZ_00250623">
        <obo:RO_0001025 rdf:resource="http://purl.obolibrary.org/obo/GAZ_00118285"/>
        <obo:IAO_0000115>An island in the Fly River Delta.</obo:IAO_0000115>
        <oboInOwl:hasOBONamespace>GAZ</oboInOwl:hasOBONamespace>
        <oboInOwl:id>GAZ:00250623</oboInOwl:id>
        <rdfs:label>Kuragimini Island</rdfs:label>
    </owl:NamedIndividual>
    


    <!-- http://purl.obolibrary.org/obo/GAZ_00250624 -->

    <owl:NamedIndividual rdf:about="http://purl.obolibrary.org/obo/GAZ_00250624">
        <obo:RO_0001025 rdf:resource="http://purl.obolibrary.org/obo/GAZ_00118285"/>
        <obo:IAO_0000115>An island in the Fly River Delta.</obo:IAO_0000115>
        <oboInOwl:hasOBONamespace>GAZ</oboInOwl:hasOBONamespace>
        <oboInOwl:id>GAZ:00250624</oboInOwl:id>
        <rdfs:label>Daura Island</rdfs:label>
    </owl:NamedIndividual>
    


    <!-- http://purl.obolibrary.org/obo/GAZ_00250625 -->

    <owl:NamedIndividual rdf:about="http://purl.obolibrary.org/obo/GAZ_00250625">
        <obo:RO_0001025 rdf:resource="http://purl.obolibrary.org/obo/GAZ_00118285"/>
        <obo:IAO_0000115>An island in the Fly River Delta.</obo:IAO_0000115>
        <oboInOwl:hasOBONamespace>GAZ</oboInOwl:hasOBONamespace>
        <oboInOwl:id>GAZ:00250625</oboInOwl:id>
        <rdfs:label>Kunagimini Islands</rdfs:label>
    </owl:NamedIndividual>
    


    <!-- http://purl.obolibrary.org/obo/GAZ_00250626 -->

    <owl:NamedIndividual rdf:about="http://purl.obolibrary.org/obo/GAZ_00250626">
        <obo:RO_0001025 rdf:resource="http://purl.obolibrary.org/obo/GAZ_00012665"/>
        <obo:IAO_0000115>A river in the Western Province of Papua New Guinea, and is the largest tributary of the Fly River.</obo:IAO_0000115>
        <oboInOwl:hasOBONamespace>GAZ</oboInOwl:hasOBONamespace>
        <oboInOwl:id>GAZ:00250626</oboInOwl:id>
        <rdfs:label>Strickland River</rdfs:label>
    </owl:NamedIndividual>
    


    <!-- http://purl.obolibrary.org/obo/GAZ_00250628 -->

    <owl:NamedIndividual rdf:about="http://purl.obolibrary.org/obo/GAZ_00250628">
        <obo:RO_0001025 rdf:resource="http://purl.obolibrary.org/obo/GAZ_00022417"/>
        <obo:IAO_0000115>A river. A tributary of the Ok Tedi River.</obo:IAO_0000115>
        <oboInOwl:hasOBONamespace>GAZ</oboInOwl:hasOBONamespace>
        <oboInOwl:id>GAZ:00250628</oboInOwl:id>
        <rdfs:label>Birim River</rdfs:label>
    </owl:NamedIndividual>
    


    <!-- http://purl.obolibrary.org/obo/GAZ_00250664 -->

    <owl:NamedIndividual rdf:about="http://purl.obolibrary.org/obo/GAZ_00250664">
        <obo:RO_0001025 rdf:resource="http://purl.obolibrary.org/obo/GAZ_00250665"/>
        <obo:IAO_0000115>A mountain range in north-eastern Papua New Guinea. The range runs into the Saruwaged Range to the east and together they form a natural barrier between the Ramu and Markham valleys to the south and Vitiaz Strait to the north. Many rivers originate in this range, including the Ramu.</obo:IAO_0000115>
        <oboInOwl:hasOBONamespace>GAZ</oboInOwl:hasOBONamespace>
        <oboInOwl:id>GAZ:00250664</oboInOwl:id>
        <rdfs:label>Finisterre Range</rdfs:label>
    </owl:NamedIndividual>
    


    <!-- http://purl.obolibrary.org/obo/GAZ_00250665 -->

    <owl:NamedIndividual rdf:about="http://purl.obolibrary.org/obo/GAZ_00250665">
        <obo:RO_0001025 rdf:resource="http://purl.obolibrary.org/obo/GAZ_00007255"/>
        <obo:IAO_0000115>A large rugged peninsula on the island of New Guinea in Morobe Province, eastern Papua New Guinea. The peninsula is dominated by the steep Saruwaged and Finisterre and Cromwell Mountains.</obo:IAO_0000115>
        <oboInOwl:hasOBONamespace>GAZ</oboInOwl:hasOBONamespace>
        <oboInOwl:id>GAZ:00250665</oboInOwl:id>
        <rdfs:label>Huon Peninsula</rdfs:label>
    </owl:NamedIndividual>
    


    <!-- http://purl.obolibrary.org/obo/GAZ_00250666 -->

    <owl:NamedIndividual rdf:about="http://purl.obolibrary.org/obo/GAZ_00250666">
        <obo:RO_0001025 rdf:resource="http://purl.obolibrary.org/obo/GAZ_00250665"/>
        <obo:IAO_0000115>A mountain range.</obo:IAO_0000115>
        <oboInOwl:hasOBONamespace>GAZ</oboInOwl:hasOBONamespace>
        <oboInOwl:id>GAZ:00250666</oboInOwl:id>
        <rdfs:label>Cromwell Mountains</rdfs:label>
    </owl:NamedIndividual>
    


    <!-- http://purl.obolibrary.org/obo/GAZ_00250667 -->

    <owl:NamedIndividual rdf:about="http://purl.obolibrary.org/obo/GAZ_00250667">
        <obo:RO_0001025 rdf:resource="http://purl.obolibrary.org/obo/GAZ_00250665"/>
        <obo:IAO_0000115>A mountain range on the Huon Peninsula in Morobe Province, north-eastern Papua New Guinea. The Saruwaged Range runs into the Finisterre Range to the west and together they form a natural barrier between the Ramu and Markham valleys to the south and Vitiaz Strait to the north.</obo:IAO_0000115>
        <oboInOwl:hasOBONamespace>GAZ</oboInOwl:hasOBONamespace>
        <oboInOwl:id>GAZ:00250667</oboInOwl:id>
        <rdfs:label>Saruwaged Range</rdfs:label>
    </owl:NamedIndividual>
    


    <!-- http://purl.obolibrary.org/obo/GAZ_00250668 -->

    <owl:NamedIndividual rdf:about="http://purl.obolibrary.org/obo/GAZ_00250668">
        <obo:RO_0001025 rdf:resource="http://purl.obolibrary.org/obo/GAZ_00005198"/>
        <obo:IAO_0000115>A river in northern Papua New Guinea. The headwaters of the river are formed in the Kratke Range from where it then travels approximately 640 km north-west to the Bismarck Sea.</obo:IAO_0000115>
        <oboInOwl:hasOBONamespace>GAZ</oboInOwl:hasOBONamespace>
        <oboInOwl:id>GAZ:00250668</oboInOwl:id>
        <rdfs:label>Ramu River</rdfs:label>
    </owl:NamedIndividual>
    


    <!-- http://purl.obolibrary.org/obo/GAZ_00250669 -->

    <owl:NamedIndividual rdf:about="http://purl.obolibrary.org/obo/GAZ_00250669">
        <obo:RO_0001025 rdf:resource="http://purl.obolibrary.org/obo/GAZ_00010064"/>
        <obo:IAO_0000115>A mountain range in Eastern Highlands, Papua New Guinea.</obo:IAO_0000115>
        <oboInOwl:hasOBONamespace>GAZ</oboInOwl:hasOBONamespace>
        <oboInOwl:id>GAZ:00250669</oboInOwl:id>
        <rdfs:label>Kratke Range</rdfs:label>
    </owl:NamedIndividual>
    


    <!-- http://purl.obolibrary.org/obo/GAZ_00250670 -->

    <owl:NamedIndividual rdf:about="http://purl.obolibrary.org/obo/GAZ_00250670">
        <obo:RO_0001025 rdf:resource="http://purl.obolibrary.org/obo/GAZ_00005198"/>
        <obo:IAO_0000115>A mountain range in Madang Province, north-central Papua New Guinea.</obo:IAO_0000115>
        <oboInOwl:hasOBONamespace>GAZ</oboInOwl:hasOBONamespace>
        <oboInOwl:id>GAZ:00250670</oboInOwl:id>
        <rdfs:label>Adelbert Range</rdfs:label>
    </owl:NamedIndividual>
    


    <!-- http://purl.obolibrary.org/obo/GAZ_00250671 -->

    <owl:NamedIndividual rdf:about="http://purl.obolibrary.org/obo/GAZ_00250671">
        <obo:RO_0001025 rdf:resource="http://purl.obolibrary.org/obo/GAZ_00005188"/>
        <obo:IAO_0000115>A mountain range in southern part of New Ireland, Papua New Guinea.</obo:IAO_0000115>
        <oboInOwl:hasOBONamespace>GAZ</oboInOwl:hasOBONamespace>
        <oboInOwl:id>GAZ:00250671</oboInOwl:id>
        <rdfs:label>Hans Meyer Range</rdfs:label>
    </owl:NamedIndividual>
    


    <!-- http://purl.obolibrary.org/obo/GAZ_00250673 -->

    <owl:NamedIndividual rdf:about="http://purl.obolibrary.org/obo/GAZ_00250673">
        <obo:RO_0001025 rdf:resource="http://purl.obolibrary.org/obo/GAZ_00005188"/>
        <obo:IAO_0000115>A mountain range in north-central part of New Ireland, Papua New Guinea.</obo:IAO_0000115>
        <oboInOwl:hasOBONamespace>GAZ</oboInOwl:hasOBONamespace>
        <oboInOwl:id>GAZ:00250673</oboInOwl:id>
        <rdfs:label>Schleinitz Range</rdfs:label>
    </owl:NamedIndividual>
    


    <!-- http://purl.obolibrary.org/obo/GAZ_00250674 -->

    <owl:NamedIndividual rdf:about="http://purl.obolibrary.org/obo/GAZ_00250674">
        <obo:RO_0001025 rdf:resource="http://purl.obolibrary.org/obo/GAZ_00250664"/>
        <obo:IAO_0000115>A razorback (stratigraphic) ridge in the Finisterre Range, in north eastern Papua New Guinea. Its highest point is 1,494 m above sea level. The ridge is located between the valleys of the Mene and Faria Rivers and culminates at one end in Kankiryo Saddle, which links it to Faria Ridge and divides Faria Valley and Mindjim River Valley.</obo:IAO_0000115>
        <oboInOwl:hasOBONamespace>GAZ</oboInOwl:hasOBONamespace>
        <oboInOwl:id>GAZ:00250674</oboInOwl:id>
        <rdfs:label>Shaggy Ridge</rdfs:label>
    </owl:NamedIndividual>
    


    <!-- http://purl.obolibrary.org/obo/GAZ_00250675 -->

    <owl:NamedIndividual rdf:about="http://purl.obolibrary.org/obo/GAZ_00250675">
        <obo:RO_0001025 rdf:resource="http://purl.obolibrary.org/obo/GAZ_00056643"/>
        <obo:IAO_0000115>A mountain range in central Papua New Guinea. It is a part of the Bismarck Range.</obo:IAO_0000115>
        <oboInOwl:hasOBONamespace>GAZ</oboInOwl:hasOBONamespace>
        <oboInOwl:id>GAZ:00250675</oboInOwl:id>
        <rdfs:label>Schrader Range</rdfs:label>
    </owl:NamedIndividual>
    


    <!-- http://purl.obolibrary.org/obo/GAZ_00250752 -->

    <owl:NamedIndividual rdf:about="http://purl.obolibrary.org/obo/GAZ_00250752">
        <obo:RO_0001025 rdf:resource="http://purl.obolibrary.org/obo/GAZ_00012665"/>
        <obo:IAO_0000115>A plateau.</obo:IAO_0000115>
        <oboInOwl:hasOBONamespace>GAZ</oboInOwl:hasOBONamespace>
        <oboInOwl:id>GAZ:00250752</oboInOwl:id>
        <rdfs:label>Oriomo Plateau</rdfs:label>
    </owl:NamedIndividual>
    


    <!-- http://purl.obolibrary.org/obo/GAZ_00253576 -->

    <owl:NamedIndividual rdf:about="http://purl.obolibrary.org/obo/GAZ_00253576">
        <obo:RO_0001025 rdf:resource="http://purl.obolibrary.org/obo/GAZ_00007255"/>
        <obo:IAO_0000115>A wetland.</obo:IAO_0000115>
        <oboInOwl:hasOBONamespace>GAZ</oboInOwl:hasOBONamespace>
        <oboInOwl:id>GAZ:00253576</oboInOwl:id>
        <rdfs:label>Markham Floodplain</rdfs:label>
    </owl:NamedIndividual>
    


    <!-- http://purl.obolibrary.org/obo/GAZ_00253578 -->

    <owl:NamedIndividual rdf:about="http://purl.obolibrary.org/obo/GAZ_00253578">
        <obo:RO_0001025 rdf:resource="http://purl.obolibrary.org/obo/GAZ_00007255"/>
        <obo:IAO_0000115>A freshwater lake. Located on the southern flank of the Markham Valley, near Oornsis, Morobe Province.</obo:IAO_0000115>
        <oboInOwl:hasOBONamespace>GAZ</oboInOwl:hasOBONamespace>
        <oboInOwl:id>GAZ:00253578</oboInOwl:id>
        <rdfs:label>Lake Wanum</rdfs:label>
    </owl:NamedIndividual>
    


    <!-- http://purl.obolibrary.org/obo/GAZ_00253579 -->

    <owl:NamedIndividual rdf:about="http://purl.obolibrary.org/obo/GAZ_00253579">
        <obo:RO_0001025 rdf:resource="http://purl.obolibrary.org/obo/GAZ_00007255"/>
        <obo:IAO_0000115>A freshwater wetland. Located on the southern flank of the Markham Valley, near Oomsis, Morobe Province.</obo:IAO_0000115>
        <oboInOwl:hasOBONamespace>GAZ</oboInOwl:hasOBONamespace>
        <oboInOwl:id>GAZ:00253579</oboInOwl:id>
        <rdfs:label>Red Hill Swamp</rdfs:label>
    </owl:NamedIndividual>
    


    <!-- http://purl.obolibrary.org/obo/GAZ_00253580 -->

    <owl:NamedIndividual rdf:about="http://purl.obolibrary.org/obo/GAZ_00253580">
        <obo:RO_0001025 rdf:resource="http://purl.obolibrary.org/obo/GAZ_00007255"/>
        <obo:IAO_0000115>A freshwater lake. Located 1 km northwest of Yatsing Village, on the southern margin of Markham River, Morobe Province.</obo:IAO_0000115>
        <oboInOwl:hasOBONamespace>GAZ</oboInOwl:hasOBONamespace>
        <oboInOwl:id>GAZ:00253580</oboInOwl:id>
        <rdfs:label>Lake Yanamugi</rdfs:label>
    </owl:NamedIndividual>
    


    <!-- http://purl.obolibrary.org/obo/GAZ_00253581 -->

    <owl:NamedIndividual rdf:about="http://purl.obolibrary.org/obo/GAZ_00253581">
        <obo:RO_0001025 rdf:resource="http://purl.obolibrary.org/obo/GAZ_00012662"/>
        <obo:IAO_0000115>A river. It rises in the north end of the Owen Stanley Range and drains northeast into the Solomon Sea near Manau.</obo:IAO_0000115>
        <oboInOwl:hasOBONamespace>GAZ</oboInOwl:hasOBONamespace>
        <oboInOwl:id>GAZ:00253581</oboInOwl:id>
        <rdfs:label>Mambare River</rdfs:label>
    </owl:NamedIndividual>
    


    <!-- http://purl.obolibrary.org/obo/GAZ_00253582 -->

    <owl:NamedIndividual rdf:about="http://purl.obolibrary.org/obo/GAZ_00253582">
        <obo:RO_0001025 rdf:resource="http://purl.obolibrary.org/obo/GAZ_00012662"/>
        <obo:IAO_0000115>A wetland. A vast area of riverine marshes and floodplain wetlands, including several small lakes, along the lower Mambare River, and extensive intertidal flats, mangrove swamps and numerous small tidal creeks in the delta.</obo:IAO_0000115>
        <oboInOwl:hasOBONamespace>GAZ</oboInOwl:hasOBONamespace>
        <oboInOwl:id>GAZ:00253582</oboInOwl:id>
        <rdfs:label>Mambare Wetland</rdfs:label>
    </owl:NamedIndividual>
    


    <!-- http://purl.obolibrary.org/obo/GAZ_00253583 -->

    <owl:NamedIndividual rdf:about="http://purl.obolibrary.org/obo/GAZ_00253583">
        <obo:RO_0001025 rdf:resource="http://purl.obolibrary.org/obo/GAZ_00012662"/>
        <obo:IAO_0000115>A wetland. A vast area of floodplain wetlands including levees and back swamps along the lower Musa River, and a large area of intertidal flats, mangrove swamps and small tidal creeks near the river mouth in Dyke Ackland Bay.</obo:IAO_0000115>
        <oboInOwl:hasOBONamespace>GAZ</oboInOwl:hasOBONamespace>
        <oboInOwl:id>GAZ:00253583</oboInOwl:id>
        <rdfs:label>Musa Wetland</rdfs:label>
    </owl:NamedIndividual>
    


    <!-- http://purl.obolibrary.org/obo/GAZ_00253584 -->

    <owl:NamedIndividual rdf:about="http://purl.obolibrary.org/obo/GAZ_00253584">
        <obo:RO_0001025 rdf:resource="http://purl.obolibrary.org/obo/GAZ_00012662"/>
        <obo:IAO_0000115>A river. Discharges to Dyke Ackland Bay.</obo:IAO_0000115>
        <oboInOwl:hasOBONamespace>GAZ</oboInOwl:hasOBONamespace>
        <oboInOwl:id>GAZ:00253584</oboInOwl:id>
        <rdfs:label>Musa River</rdfs:label>
    </owl:NamedIndividual>
    


    <!-- http://purl.obolibrary.org/obo/GAZ_00253585 -->

    <owl:NamedIndividual rdf:about="http://purl.obolibrary.org/obo/GAZ_00253585">
        <obo:RO_0001025 rdf:resource="http://purl.obolibrary.org/obo/GAZ_00012662"/>
        <obo:IAO_0000115>A bay.</obo:IAO_0000115>
        <oboInOwl:hasOBONamespace>GAZ</oboInOwl:hasOBONamespace>
        <oboInOwl:id>GAZ:00253585</oboInOwl:id>
        <rdfs:label>Dyke Ackland Bay</rdfs:label>
    </owl:NamedIndividual>
    


    <!-- http://purl.obolibrary.org/obo/GAZ_00253586 -->

    <owl:NamedIndividual rdf:about="http://purl.obolibrary.org/obo/GAZ_00253586">
        <obo:RO_0001025 rdf:resource="http://purl.obolibrary.org/obo/GAZ_00016855"/>
        <obo:IAO_0000115>A freshwater lake. Located in the interior of Fergusson Island.</obo:IAO_0000115>
        <oboInOwl:hasOBONamespace>GAZ</oboInOwl:hasOBONamespace>
        <oboInOwl:id>GAZ:00253586</oboInOwl:id>
        <rdfs:label>Lake Lavu</rdfs:label>
    </owl:NamedIndividual>
    


    <!-- http://purl.obolibrary.org/obo/GAZ_00253587 -->

    <owl:NamedIndividual rdf:about="http://purl.obolibrary.org/obo/GAZ_00253587">
        <obo:RO_0001025 rdf:resource="http://purl.obolibrary.org/obo/GAZ_00016856"/>
        <obo:IAO_0000115>A protected area. Comprises mangrove swamps around a small bay on the north coast of Normanby Island, with seasonal slow-flowing streams, swampy areas, seasonally flooded grassland and swamp forest inland. Established 1977.</obo:IAO_0000115>
        <oboInOwl:hasOBONamespace>GAZ</oboInOwl:hasOBONamespace>
        <oboInOwl:id>GAZ:00253587</oboInOwl:id>
        <rdfs:label>Sawataetae Wildlife Management Area</rdfs:label>
    </owl:NamedIndividual>
    


    <!-- http://purl.obolibrary.org/obo/GAZ_00253588 -->

    <owl:NamedIndividual rdf:about="http://purl.obolibrary.org/obo/GAZ_00253588">
        <obo:RO_0001025 rdf:resource="http://purl.obolibrary.org/obo/GAZ_00012666"/>
        <obo:IAO_0000115>A wetland. Located at the west end of Mime Bay, near the southeastern extremity of the PNG mainland, Milne Bay Province.</obo:IAO_0000115>
        <oboInOwl:hasOBONamespace>GAZ</oboInOwl:hasOBONamespace>
        <oboInOwl:id>GAZ:00253588</oboInOwl:id>
        <rdfs:label>Rakua Wetland</rdfs:label>
    </owl:NamedIndividual>
    


    <!-- http://purl.obolibrary.org/obo/GAZ_00253589 -->

    <owl:NamedIndividual rdf:about="http://purl.obolibrary.org/obo/GAZ_00253589">
        <obo:RO_0001025 rdf:resource="http://purl.obolibrary.org/obo/GAZ_00012666"/>
        <obo:IAO_0000115>A bay.</obo:IAO_0000115>
        <oboInOwl:hasOBONamespace>GAZ</oboInOwl:hasOBONamespace>
        <oboInOwl:id>GAZ:00253589</oboInOwl:id>
        <rdfs:label>Mullins Harbour</rdfs:label>
    </owl:NamedIndividual>
    


    <!-- http://purl.obolibrary.org/obo/GAZ_00253590 -->

    <owl:NamedIndividual rdf:about="http://purl.obolibrary.org/obo/GAZ_00253590">
        <obo:RO_0001025 rdf:resource="http://purl.obolibrary.org/obo/GAZ_00012666"/>
        <obo:IAO_0000115>A wetland around Mullins Harbour. Located 30 km WSW of Milne Bay, Milne Bay Province.</obo:IAO_0000115>
        <oboInOwl:hasOBONamespace>GAZ</oboInOwl:hasOBONamespace>
        <oboInOwl:id>GAZ:00253590</oboInOwl:id>
        <rdfs:label>Mullins Harbour Wetland</rdfs:label>
    </owl:NamedIndividual>
    


    <!-- http://purl.obolibrary.org/obo/GAZ_00253591 -->

    <owl:NamedIndividual rdf:about="http://purl.obolibrary.org/obo/GAZ_00253591">
        <obo:RO_0001025 rdf:resource="http://purl.obolibrary.org/obo/GAZ_00012657"/>
        <obo:IAO_0000115>A lake. Located 110 km NW of Port Moresby.</obo:IAO_0000115>
        <oboInOwl:hasOBONamespace>GAZ</oboInOwl:hasOBONamespace>
        <oboInOwl:id>GAZ:00253591</oboInOwl:id>
        <rdfs:label>Lake Kumu</rdfs:label>
    </owl:NamedIndividual>
    


    <!-- http://purl.obolibrary.org/obo/GAZ_00253592 -->

    <owl:NamedIndividual rdf:about="http://purl.obolibrary.org/obo/GAZ_00253592">
        <obo:RO_0001025 rdf:resource="http://purl.obolibrary.org/obo/GAZ_00012657"/>
        <obo:IAO_0000115>Wetlands. They extend from the Port Moresby area northwest for about 50 km, and include the lower regions and estuaries of the Vanapa, Brown, Laloki, Aroa, Kubuna and Kuriva rivers.</obo:IAO_0000115>
        <oboInOwl:hasOBONamespace>GAZ</oboInOwl:hasOBONamespace>
        <oboInOwl:id>GAZ:00253592</oboInOwl:id>
        <rdfs:label>Vanapa Wetlands</rdfs:label>
    </owl:NamedIndividual>
    


    <!-- http://purl.obolibrary.org/obo/GAZ_00253593 -->

    <owl:NamedIndividual rdf:about="http://purl.obolibrary.org/obo/GAZ_00253593">
        <obo:RO_0001025 rdf:resource="http://purl.obolibrary.org/obo/GAZ_00012657"/>
        <obo:IAO_0000115>Wetlands. Located 100 km southeast of Port Moresby) comprise the floodplain and estuarine marshes of the Kemp Welch River and coastal mangrove swamps to the east.</obo:IAO_0000115>
        <oboInOwl:hasOBONamespace>GAZ</oboInOwl:hasOBONamespace>
        <oboInOwl:id>GAZ:00253593</oboInOwl:id>
        <rdfs:label>Kemp Welch Wetlands</rdfs:label>
    </owl:NamedIndividual>
    


    <!-- http://purl.obolibrary.org/obo/GAZ_00253594 -->

    <owl:NamedIndividual rdf:about="http://purl.obolibrary.org/obo/GAZ_00253594">
        <obo:RO_0001025 rdf:resource="http://purl.obolibrary.org/obo/GAZ_00012657"/>
        <obo:IAO_0000115>A wetland. Located 185 km southeast of Port Moresby) include the floodplain and estuarine marshes of the Mon River and the mangrove swamps lining the bay to the east.</obo:IAO_0000115>
        <oboInOwl:hasOBONamespace>GAZ</oboInOwl:hasOBONamespace>
        <oboInOwl:id>GAZ:00253594</oboInOwl:id>
        <rdfs:label>Mon Wetlands</rdfs:label>
    </owl:NamedIndividual>
    


    <!-- http://purl.obolibrary.org/obo/GAZ_00253603 -->

    <owl:NamedIndividual rdf:about="http://purl.obolibrary.org/obo/GAZ_00253603">
        <obo:RO_0001025 rdf:resource="http://purl.obolibrary.org/obo/GAZ_00012657"/>
        <obo:IAO_0000115>A wetland. A complex of shallow, eutrophic, freshwater lakes and surrounding swamps associated with the Laloki River. Located 15 km north of Port Moresby, National Capital District.</obo:IAO_0000115>
        <oboInOwl:hasOBONamespace>GAZ</oboInOwl:hasOBONamespace>
        <oboInOwl:id>GAZ:00253603</oboInOwl:id>
        <rdfs:label>Waigani Swamp</rdfs:label>
    </owl:NamedIndividual>
    


    <!-- http://purl.obolibrary.org/obo/GAZ_00253604 -->

    <owl:NamedIndividual rdf:about="http://purl.obolibrary.org/obo/GAZ_00253604">
        <obo:RO_0001025 rdf:resource="http://purl.obolibrary.org/obo/GAZ_00012657"/>
        <obo:IAO_0000115>A wetland. Comprieses an area of intertidal sand and mud flats with a complex of mangrove swamps, salt flats and sandy beach ridges. Parts of the wetland are subject to seasonal flooding with brackish water. Located about 30 km northwest of Port Moresby, Central Province.</obo:IAO_0000115>
        <oboInOwl:hasOBONamespace>GAZ</oboInOwl:hasOBONamespace>
        <oboInOwl:id>GAZ:00253604</oboInOwl:id>
        <rdfs:label>Lea Lea Salt Flats</rdfs:label>
    </owl:NamedIndividual>
    


    <!-- http://purl.obolibrary.org/obo/GAZ_00253605 -->

    <owl:NamedIndividual rdf:about="http://purl.obolibrary.org/obo/GAZ_00253605">
        <obo:RO_0001025 rdf:resource="http://purl.obolibrary.org/obo/GAZ_00005198"/>
        <obo:IAO_0000115>A river in Madang Province, Papua New Guinea. It rises in the Adelbert Range and empties to the Bismarck Sea.</obo:IAO_0000115>
        <oboInOwl:hasOBONamespace>GAZ</oboInOwl:hasOBONamespace>
        <oboInOwl:id>GAZ:00253605</oboInOwl:id>
        <rdfs:label>Malas River</rdfs:label>
    </owl:NamedIndividual>
    


    <!-- http://purl.obolibrary.org/obo/GAZ_00253606 -->

    <owl:NamedIndividual rdf:about="http://purl.obolibrary.org/obo/GAZ_00253606">
        <obo:RO_0001025 rdf:resource="http://purl.obolibrary.org/obo/GAZ_00012662"/>
        <obo:IAO_0000115>A river located in the Northern Province of Papua New Guinea.</obo:IAO_0000115>
        <oboInOwl:hasOBONamespace>GAZ</oboInOwl:hasOBONamespace>
        <oboInOwl:id>GAZ:00253606</oboInOwl:id>
        <rdfs:label>Kumusi River</rdfs:label>
    </owl:NamedIndividual>
    


    <!-- http://purl.obolibrary.org/obo/GAZ_00253607 -->

    <owl:NamedIndividual rdf:about="http://purl.obolibrary.org/obo/GAZ_00253607">
        <obo:RO_0001025 rdf:resource="http://purl.obolibrary.org/obo/GAZ_00012659"/>
        <obo:IAO_0000115>A river in that originates in the south central highlands of Papua New Guinea, flowing 470 km though the Gulf Province to the Gulf of Papua.</obo:IAO_0000115>
        <oboInOwl:hasOBONamespace>GAZ</oboInOwl:hasOBONamespace>
        <oboInOwl:id>GAZ:00253607</oboInOwl:id>
        <rdfs:label>Purari River</rdfs:label>
    </owl:NamedIndividual>
    


    <!-- http://purl.obolibrary.org/obo/GAZ_00253612 -->

    <owl:NamedIndividual rdf:about="http://purl.obolibrary.org/obo/GAZ_00253612">
        <obo:RO_0001025 rdf:resource="http://purl.obolibrary.org/obo/GAZ_00005198"/>
        <obo:IAO_0000115>A river in Madang Province, Papua New Guinea.</obo:IAO_0000115>
        <oboInOwl:hasOBONamespace>GAZ</oboInOwl:hasOBONamespace>
        <oboInOwl:id>GAZ:00253612</oboInOwl:id>
        <rdfs:label>Sogeram River</rdfs:label>
    </owl:NamedIndividual>
    


    <!-- http://purl.obolibrary.org/obo/GAZ_00253613 -->

    <owl:NamedIndividual rdf:about="http://purl.obolibrary.org/obo/GAZ_00253613">
        <obo:RO_0001025 rdf:resource="http://purl.obolibrary.org/obo/GAZ_00005184"/>
        <obo:IAO_0000115>A river in Bougainville, Papua New Guinea. It empties to Empress Augusta Bay.</obo:IAO_0000115>
        <oboInOwl:hasOBONamespace>GAZ</oboInOwl:hasOBONamespace>
        <oboInOwl:id>GAZ:00253613</oboInOwl:id>
        <rdfs:label>Torokina River</rdfs:label>
    </owl:NamedIndividual>
    


    <!-- http://purl.obolibrary.org/obo/GAZ_00253614 -->

    <owl:NamedIndividual rdf:about="http://purl.obolibrary.org/obo/GAZ_00253614">
        <obo:RO_0001025 rdf:resource="http://purl.obolibrary.org/obo/GAZ_00012659"/>
        <obo:IAO_0000115>A river.</obo:IAO_0000115>
        <oboInOwl:hasOBONamespace>GAZ</oboInOwl:hasOBONamespace>
        <oboInOwl:id>GAZ:00253614</oboInOwl:id>
        <rdfs:label>Turama River</rdfs:label>
    </owl:NamedIndividual>
    


    <!-- http://purl.obolibrary.org/obo/GAZ_00253616 -->

    <owl:NamedIndividual rdf:about="http://purl.obolibrary.org/obo/GAZ_00253616">
        <obo:RO_0001025 rdf:resource="http://purl.obolibrary.org/obo/GAZ_00007255"/>
        <obo:IAO_0000115>A river in Morobe Province, Papua New Guinea.</obo:IAO_0000115>
        <oboInOwl:hasOBONamespace>GAZ</oboInOwl:hasOBONamespace>
        <oboInOwl:id>GAZ:00253616</oboInOwl:id>
        <rdfs:label>Watut River</rdfs:label>
    </owl:NamedIndividual>
    


    <!-- http://purl.obolibrary.org/obo/GAZ_00253617 -->

    <owl:NamedIndividual rdf:about="http://purl.obolibrary.org/obo/GAZ_00253617">
        <obo:RO_0001025 rdf:resource="http://purl.obolibrary.org/obo/GAZ_00012665"/>
        <obo:IAO_0000115>A river.</obo:IAO_0000115>
        <oboInOwl:hasOBONamespace>GAZ</oboInOwl:hasOBONamespace>
        <oboInOwl:id>GAZ:00253617</oboInOwl:id>
        <rdfs:label>Wawoi River</rdfs:label>
    </owl:NamedIndividual>
    


    <!-- http://purl.obolibrary.org/obo/GAZ_00253618 -->

    <owl:NamedIndividual rdf:about="http://purl.obolibrary.org/obo/GAZ_00253618">
        <obo:RO_0001025 rdf:resource="http://purl.obolibrary.org/obo/GAZ_00005192"/>
        <obo:IAO_0000115>A river.</obo:IAO_0000115>
        <oboInOwl:hasOBONamespace>GAZ</oboInOwl:hasOBONamespace>
        <oboInOwl:id>GAZ:00253618</oboInOwl:id>
        <rdfs:label>Nengmutka River</rdfs:label>
    </owl:NamedIndividual>
    


    <!-- http://purl.obolibrary.org/obo/GAZ_00253619 -->

    <owl:NamedIndividual rdf:about="http://purl.obolibrary.org/obo/GAZ_00253619">
        <obo:RO_0001025 rdf:resource="http://purl.obolibrary.org/obo/GAZ_00010064"/>
        <obo:IAO_0000115>A river in Eastern Highlands province, Papua New Guinea.</obo:IAO_0000115>
        <oboInOwl:hasOBONamespace>GAZ</oboInOwl:hasOBONamespace>
        <oboInOwl:id>GAZ:00253619</oboInOwl:id>
        <rdfs:label>Asaro River</rdfs:label>
    </owl:NamedIndividual>
    


    <!-- http://purl.obolibrary.org/obo/GAZ_00253620 -->

    <owl:NamedIndividual rdf:about="http://purl.obolibrary.org/obo/GAZ_00253620">
        <obo:RO_0001025 rdf:resource="http://purl.obolibrary.org/obo/GAZ_00012658"/>
        <obo:IAO_0000115>A river.</obo:IAO_0000115>
        <oboInOwl:hasOBONamespace>GAZ</oboInOwl:hasOBONamespace>
        <oboInOwl:id>GAZ:00253620</oboInOwl:id>
        <rdfs:label>Chimbu River</rdfs:label>
    </owl:NamedIndividual>
    


    <!-- http://purl.obolibrary.org/obo/GAZ_00253621 -->

    <owl:NamedIndividual rdf:about="http://purl.obolibrary.org/obo/GAZ_00253621">
        <obo:RO_0001025 rdf:resource="http://purl.obolibrary.org/obo/GAZ_00005198"/>
        <obo:IAO_0000115>A river in Madang Province, Papua New Guinea. It empties to Astrolabe Bay.</obo:IAO_0000115>
        <oboInOwl:hasOBONamespace>GAZ</oboInOwl:hasOBONamespace>
        <oboInOwl:id>GAZ:00253621</oboInOwl:id>
        <rdfs:label>Gogol River</rdfs:label>
    </owl:NamedIndividual>
    


    <!-- http://purl.obolibrary.org/obo/GAZ_00253622 -->

    <owl:NamedIndividual rdf:about="http://purl.obolibrary.org/obo/GAZ_00253622">
        <obo:RO_0001025 rdf:resource="http://purl.obolibrary.org/obo/GAZ_00005184"/>
        <obo:IAO_0000115>A river in Bougainville, Papua New Guinea. It empties to Empress Augusta Bay.</obo:IAO_0000115>
        <oboInOwl:hasOBONamespace>GAZ</oboInOwl:hasOBONamespace>
        <oboInOwl:id>GAZ:00253622</oboInOwl:id>
        <rdfs:label>Jaba River</rdfs:label>
    </owl:NamedIndividual>
    


    <!-- http://purl.obolibrary.org/obo/GAZ_00253623 -->

    <owl:NamedIndividual rdf:about="http://purl.obolibrary.org/obo/GAZ_00253623">
        <obo:RO_0001025 rdf:resource="http://purl.obolibrary.org/obo/GAZ_00005198"/>
        <obo:IAO_0000115>A river in Madang Province, Papua New Guinea. It flows westward and empties near Rimba to the Astrolabe Bay.</obo:IAO_0000115>
        <oboInOwl:hasOBONamespace>GAZ</oboInOwl:hasOBONamespace>
        <oboInOwl:id>GAZ:00253623</oboInOwl:id>
        <rdfs:label>Kabenau River</rdfs:label>
    </owl:NamedIndividual>
    


    <!-- http://purl.obolibrary.org/obo/GAZ_00253624 -->

    <owl:NamedIndividual rdf:about="http://purl.obolibrary.org/obo/GAZ_00253624">
        <obo:RO_0001025 rdf:resource="http://purl.obolibrary.org/obo/GAZ_00012659"/>
        <obo:IAO_0000115>A river that flows southeast into the Gulf of Papua, with its delta at the head of the gulf.</obo:IAO_0000115>
        <oboInOwl:hasOBONamespace>GAZ</oboInOwl:hasOBONamespace>
        <oboInOwl:id>GAZ:00253624</oboInOwl:id>
        <rdfs:label>Kikori River</rdfs:label>
    </owl:NamedIndividual>
    


    <!-- http://purl.obolibrary.org/obo/GAZ_00253625 -->

    <owl:NamedIndividual rdf:about="http://purl.obolibrary.org/obo/GAZ_00253625">
        <obo:RO_0001025 rdf:resource="http://purl.obolibrary.org/obo/GAZ_00005184"/>
        <obo:IAO_0000115>A narrow peninsula located on Bougainville Island, Papua New Guinea, at the north of the island. The Buka Passage separates the peninsula from Buka Island.</obo:IAO_0000115>
        <oboInOwl:hasOBONamespace>GAZ</oboInOwl:hasOBONamespace>
        <oboInOwl:id>GAZ:00253625</oboInOwl:id>
        <rdfs:label>Bonis Peninsula</rdfs:label>
    </owl:NamedIndividual>
    


    <!-- http://purl.obolibrary.org/obo/GAZ_00253626 -->

    <owl:NamedIndividual rdf:about="http://purl.obolibrary.org/obo/GAZ_00253626">
        <obo:RO_0001025 rdf:resource="http://purl.obolibrary.org/obo/GAZ_00016849"/>
        <obo:IAO_0000115>A mountain range.</obo:IAO_0000115>
        <oboInOwl:hasOBONamespace>GAZ</oboInOwl:hasOBONamespace>
        <oboInOwl:id>GAZ:00253626</oboInOwl:id>
        <rdfs:label>Richard Parkinson Range</rdfs:label>
    </owl:NamedIndividual>
    


    <!-- http://purl.obolibrary.org/obo/GAZ_00253627 -->

    <owl:NamedIndividual rdf:about="http://purl.obolibrary.org/obo/GAZ_00253627">
        <obo:RO_0001025 rdf:resource="http://purl.obolibrary.org/obo/GAZ_00016849"/>
        <obo:IAO_0000115>A river.</obo:IAO_0000115>
        <oboInOwl:hasOBONamespace>GAZ</oboInOwl:hasOBONamespace>
        <oboInOwl:id>GAZ:00253627</oboInOwl:id>
        <rdfs:label>Gagan River</rdfs:label>
    </owl:NamedIndividual>
    


    <!-- http://purl.obolibrary.org/obo/GAZ_00253628 -->

    <owl:NamedIndividual rdf:about="http://purl.obolibrary.org/obo/GAZ_00253628">
        <obo:RO_0001025 rdf:resource="http://purl.obolibrary.org/obo/GAZ_00012666"/>
        <obo:IAO_0000115>A navigable strait in the Milne Bay Province of Papua New Guinea between the Louisiade Archipelago and New Guinea. The channel lies between the Jomard Islands and Duperre Islets and connects the Solomon Sea with the Coral Sea.</obo:IAO_0000115>
        <oboInOwl:hasOBONamespace>GAZ</oboInOwl:hasOBONamespace>
        <oboInOwl:id>GAZ:00253628</oboInOwl:id>
        <rdfs:label>Jomard Channel</rdfs:label>
    </owl:NamedIndividual>
    


    <!-- http://purl.obolibrary.org/obo/GAZ_00253630 -->

    <owl:NamedIndividual rdf:about="http://purl.obolibrary.org/obo/GAZ_00253630">
        <obo:RO_0001025 rdf:resource="http://purl.obolibrary.org/obo/GAZ_00012657"/>
        <obo:IAO_0000115>An inlet located in southeastern Papua New Guinea, south of Port Moresby.</obo:IAO_0000115>
        <oboInOwl:hasOBONamespace>GAZ</oboInOwl:hasOBONamespace>
        <oboInOwl:id>GAZ:00253630</oboInOwl:id>
        <rdfs:label>Bootless Inlet</rdfs:label>
    </owl:NamedIndividual>
    


    <!-- http://purl.obolibrary.org/obo/GAZ_00253632 -->

    <owl:NamedIndividual rdf:about="http://purl.obolibrary.org/obo/GAZ_00253632">
        <obo:RO_0001025 rdf:resource="http://purl.obolibrary.org/obo/GAZ_00012662"/>
        <obo:IAO_0000115>A wetland in Northern Province, Papua New Guinea.</obo:IAO_0000115>
        <oboInOwl:hasOBONamespace>GAZ</oboInOwl:hasOBONamespace>
        <oboInOwl:id>GAZ:00253632</oboInOwl:id>
        <rdfs:label>Agaiambo</rdfs:label>
    </owl:NamedIndividual>
    


    <!-- http://purl.obolibrary.org/obo/GAZ_00253633 -->

    <owl:NamedIndividual rdf:about="http://purl.obolibrary.org/obo/GAZ_00253633">
        <obo:RO_0001025 rdf:resource="http://purl.obolibrary.org/obo/GAZ_00022398"/>
        <obo:IAO_0000115>A remote submerged coral atoll, about 40 km in diameter, extending over an area of 1300 km2, located approximately 200 km northeast of New Ireland in the Bismarck Archipelago of Papua New Guinea, and 150 km northeast of Simberi Island, the closest island.</obo:IAO_0000115>
        <oboInOwl:hasOBONamespace>GAZ</oboInOwl:hasOBONamespace>
        <oboInOwl:id>GAZ:00253633</oboInOwl:id>
        <rdfs:label>Lyra Reef</rdfs:label>
    </owl:NamedIndividual>
    


    <!-- http://purl.obolibrary.org/obo/GAZ_00253634 -->

    <owl:NamedIndividual rdf:about="http://purl.obolibrary.org/obo/GAZ_00253634">
        <rdf:type rdf:resource="http://purl.obolibrary.org/obo/ENVO_00000305"/>
        <obo:RO_0001025 rdf:resource="http://purl.obolibrary.org/obo/GAZ_00012662"/>
        <obo:IAO_0000115>A cape on the north coast of Northern Province, Papua New Guinea.</obo:IAO_0000115>
        <oboInOwl:hasOBONamespace>GAZ</oboInOwl:hasOBONamespace>
        <oboInOwl:id>GAZ:00253634</oboInOwl:id>
        <rdfs:label>Cape Ward Hunt</rdfs:label>
    </owl:NamedIndividual>
    


    <!-- http://purl.obolibrary.org/obo/GAZ_00253636 -->

    <owl:NamedIndividual rdf:about="http://purl.obolibrary.org/obo/GAZ_00253636">
        <obo:RO_0001025 rdf:resource="http://purl.obolibrary.org/obo/GAZ_00012666"/>
        <obo:IAO_0000115>A navigable strait in the Milne Bay Province of Papua New Guinea between Samarai Island and Sariba Island. The strait connects the Solomon Sea with the Coral Sea.</obo:IAO_0000115>
        <oboInOwl:hasOBONamespace>GAZ</oboInOwl:hasOBONamespace>
        <oboInOwl:id>GAZ:00253636</oboInOwl:id>
        <rdfs:label>China Strait</rdfs:label>
    </owl:NamedIndividual>
    


    <!-- http://purl.obolibrary.org/obo/GAZ_00253638 -->

    <owl:NamedIndividual rdf:about="http://purl.obolibrary.org/obo/GAZ_00253638">
        <obo:RO_0001025 rdf:resource="http://purl.obolibrary.org/obo/GAZ_00012662"/>
        <obo:IAO_0000115>A bay.</obo:IAO_0000115>
        <oboInOwl:hasOBONamespace>GAZ</oboInOwl:hasOBONamespace>
        <oboInOwl:id>GAZ:00253638</oboInOwl:id>
        <rdfs:label>Collingwood Bay</rdfs:label>
    </owl:NamedIndividual>
    


    <!-- http://purl.obolibrary.org/obo/GAZ_00253639 -->

    <owl:NamedIndividual rdf:about="http://purl.obolibrary.org/obo/GAZ_00253639">
        <obo:RO_0001025 rdf:resource="http://purl.obolibrary.org/obo/GAZ_00012664"/>
        <obo:IAO_0000115>A cave.</obo:IAO_0000115>
        <oboInOwl:hasOBONamespace>GAZ</oboInOwl:hasOBONamespace>
        <oboInOwl:id>GAZ:00253639</oboInOwl:id>
        <rdfs:label>Atea Kananda Cave</rdfs:label>
    </owl:NamedIndividual>
    


    <!-- http://purl.obolibrary.org/obo/GAZ_00253640 -->

    <owl:NamedIndividual rdf:about="http://purl.obolibrary.org/obo/GAZ_00253640">
        <obo:RO_0001025 rdf:resource="http://purl.obolibrary.org/obo/GAZ_00005189"/>
    </owl:NamedIndividual>
    


    <!-- http://purl.obolibrary.org/obo/GAZ_00253642 -->

    <owl:NamedIndividual rdf:about="http://purl.obolibrary.org/obo/GAZ_00253642">
        <obo:RO_0001025 rdf:resource="http://purl.obolibrary.org/obo/GAZ_00053954"/>
        <obo:IAO_0000115>A crater lake.</obo:IAO_0000115>
        <oboInOwl:hasOBONamespace>GAZ</oboInOwl:hasOBONamespace>
        <oboInOwl:id>GAZ:00253642</oboInOwl:id>
        <rdfs:label>Loloru Lake</rdfs:label>
    </owl:NamedIndividual>
    


    <!-- http://purl.obolibrary.org/obo/GAZ_00253643 -->

    <owl:NamedIndividual rdf:about="http://purl.obolibrary.org/obo/GAZ_00253643">
        <obo:RO_0001025 rdf:resource="http://purl.obolibrary.org/obo/GAZ_00058484"/>
        <obo:IAO_0000115>An island.</obo:IAO_0000115>
        <oboInOwl:hasOBONamespace>GAZ</oboInOwl:hasOBONamespace>
        <oboInOwl:id>GAZ:00253643</oboInOwl:id>
        <rdfs:label>Wasemi Island</rdfs:label>
    </owl:NamedIndividual>
    


    <!-- http://purl.obolibrary.org/obo/GAZ_00253644 -->

    <owl:NamedIndividual rdf:about="http://purl.obolibrary.org/obo/GAZ_00253644">
        <obo:RO_0001025 rdf:resource="http://purl.obolibrary.org/obo/GAZ_00053950"/>
        <obo:IAO_0000115>A crater lake.</obo:IAO_0000115>
        <oboInOwl:hasOBONamespace>GAZ</oboInOwl:hasOBONamespace>
        <oboInOwl:id>GAZ:00253644</oboInOwl:id>
        <rdfs:label>Billy Mitchell Lake</rdfs:label>
    </owl:NamedIndividual>
    


    <!-- http://purl.obolibrary.org/obo/GAZ_00253645 -->

    <owl:NamedIndividual rdf:about="http://purl.obolibrary.org/obo/GAZ_00253645">
        <obo:RO_0001025 rdf:resource="http://purl.obolibrary.org/obo/GAZ_00012657"/>
        <obo:IAO_0000115>Three shallow freshwater lakes which sometimes unite to form a single large lake, on the flood plain of the Laloki and Brown Rivers. Located about 28 km northwest of Port Moresby, Central Province.</obo:IAO_0000115>
        <oboInOwl:hasOBONamespace>GAZ</oboInOwl:hasOBONamespace>
        <oboInOwl:id>GAZ:00253645</oboInOwl:id>
        <rdfs:label>Lake Laraguma</rdfs:label>
    </owl:NamedIndividual>
    


    <!-- http://purl.obolibrary.org/obo/GAZ_00253646 -->

    <owl:NamedIndividual rdf:about="http://purl.obolibrary.org/obo/GAZ_00253646">
        <obo:RO_0001025 rdf:resource="http://purl.obolibrary.org/obo/GAZ_00012657"/>
        <obo:IAO_0000115>A shallow freshwater lagoon. Located about 55 km northwest of Port Moresby, Central Province.</obo:IAO_0000115>
        <oboInOwl:hasOBONamespace>GAZ</oboInOwl:hasOBONamespace>
        <oboInOwl:id>GAZ:00253646</oboInOwl:id>
        <rdfs:label>Kanosia Lagoon</rdfs:label>
    </owl:NamedIndividual>
    


    <!-- http://purl.obolibrary.org/obo/GAZ_00253647 -->

    <owl:NamedIndividual rdf:about="http://purl.obolibrary.org/obo/GAZ_00253647">
        <obo:RO_0001025 rdf:resource="http://purl.obolibrary.org/obo/GAZ_00012657"/>
        <obo:IAO_0000115>A large freshwater lagoon. Located about 65 km northwest of Port Moresby, Central Province.</obo:IAO_0000115>
        <oboInOwl:hasOBONamespace>GAZ</oboInOwl:hasOBONamespace>
        <oboInOwl:id>GAZ:00253647</oboInOwl:id>
        <rdfs:label>Aroa Lagoon</rdfs:label>
    </owl:NamedIndividual>
    


    <!-- http://purl.obolibrary.org/obo/GAZ_00253648 -->

    <owl:NamedIndividual rdf:about="http://purl.obolibrary.org/obo/GAZ_00253648">
        <obo:RO_0001025 rdf:resource="http://purl.obolibrary.org/obo/GAZ_00012657"/>
        <obo:IAO_0000115>A shallow freshwater lagoon. Located about 65 km northwest of Port Moresby, Central Province.</obo:IAO_0000115>
        <oboInOwl:hasOBONamespace>GAZ</oboInOwl:hasOBONamespace>
        <oboInOwl:id>GAZ:00253648</oboInOwl:id>
        <rdfs:label>Hisiu Lagoon</rdfs:label>
    </owl:NamedIndividual>
    


    <!-- http://purl.obolibrary.org/obo/GAZ_00253649 -->

    <owl:NamedIndividual rdf:about="http://purl.obolibrary.org/obo/GAZ_00253649">
        <obo:RO_0001025 rdf:resource="http://purl.obolibrary.org/obo/GAZ_00146248"/>
        <obo:IAO_0000115>A bay.</obo:IAO_0000115>
        <oboInOwl:hasOBONamespace>GAZ</oboInOwl:hasOBONamespace>
        <oboInOwl:id>GAZ:00253649</oboInOwl:id>
        <rdfs:label>Deception Bay</rdfs:label>
    </owl:NamedIndividual>
    


    <!-- http://purl.obolibrary.org/obo/GAZ_00253650 -->

    <owl:NamedIndividual rdf:about="http://purl.obolibrary.org/obo/GAZ_00253650">
        <obo:RO_0001025 rdf:resource="http://purl.obolibrary.org/obo/GAZ_00012659"/>
        <obo:IAO_0000115>Wetlands. The coastal lowlands of Gulf Province from the mouth of the Turama River to the delta of the Purari River on Deception Bay, Gulf Province.</obo:IAO_0000115>
        <oboInOwl:hasOBONamespace>GAZ</oboInOwl:hasOBONamespace>
        <oboInOwl:id>GAZ:00253650</oboInOwl:id>
        <rdfs:label>Kikori Wetlands</rdfs:label>
    </owl:NamedIndividual>
    


    <!-- http://purl.obolibrary.org/obo/GAZ_00253651 -->

    <owl:NamedIndividual rdf:about="http://purl.obolibrary.org/obo/GAZ_00253651">
        <obo:RO_0001025 rdf:resource="http://purl.obolibrary.org/obo/GAZ_00012665"/>
        <obo:IAO_0000115>A wetland. Located from the region of Kiunga near the foothills of the Victor Emanuel Range on the Irian Jaya border, south to the Fly River Delta in the Gulf of Papua, Western Province.</obo:IAO_0000115>
        <oboInOwl:hasOBONamespace>GAZ</oboInOwl:hasOBONamespace>
        <oboInOwl:id>GAZ:00253651</oboInOwl:id>
        <rdfs:label>Fly River Floodplain</rdfs:label>
    </owl:NamedIndividual>
    


    <!-- http://purl.obolibrary.org/obo/GAZ_00253652 -->

    <owl:NamedIndividual rdf:about="http://purl.obolibrary.org/obo/GAZ_00253652">
        <obo:RO_0001025 rdf:resource="http://purl.obolibrary.org/obo/GAZ_00253651"/>
        <obo:IAO_0000115>A lake.</obo:IAO_0000115>
        <oboInOwl:hasOBONamespace>GAZ</oboInOwl:hasOBONamespace>
        <oboInOwl:id>GAZ:00253652</oboInOwl:id>
        <rdfs:label>Lake Nangamange</rdfs:label>
    </owl:NamedIndividual>
    


    <!-- http://purl.obolibrary.org/obo/GAZ_00253653 -->

    <owl:NamedIndividual rdf:about="http://purl.obolibrary.org/obo/GAZ_00253653">
        <obo:RO_0001025 rdf:resource="http://purl.obolibrary.org/obo/GAZ_00253651"/>
        <obo:IAO_0000115>A lake.</obo:IAO_0000115>
        <oboInOwl:hasOBONamespace>GAZ</oboInOwl:hasOBONamespace>
        <oboInOwl:id>GAZ:00253653</oboInOwl:id>
        <rdfs:label>Szaga Lake</rdfs:label>
    </owl:NamedIndividual>
    


    <!-- http://purl.obolibrary.org/obo/GAZ_00253654 -->

    <owl:NamedIndividual rdf:about="http://purl.obolibrary.org/obo/GAZ_00253654">
        <obo:RO_0001025 rdf:resource="http://purl.obolibrary.org/obo/GAZ_00253651"/>
        <obo:IAO_0000115>A lake.</obo:IAO_0000115>
        <oboInOwl:hasOBONamespace>GAZ</oboInOwl:hasOBONamespace>
        <oboInOwl:id>GAZ:00253654</oboInOwl:id>
        <rdfs:label>Khanda Lake</rdfs:label>
    </owl:NamedIndividual>
    


    <!-- http://purl.obolibrary.org/obo/GAZ_00253655 -->

    <owl:NamedIndividual rdf:about="http://purl.obolibrary.org/obo/GAZ_00253655">
        <obo:RO_0001025 rdf:resource="http://purl.obolibrary.org/obo/GAZ_00253651"/>
        <obo:IAO_0000115>A lake. Located on the west bank of the Fly River, 120 km SSW of Kiunga, Western Province. A lateral lake formed by a tributary stream being blocked through accretion by the Fly River. The lake is connected to the Fly River by a narrow channel 5m wide.</obo:IAO_0000115>
        <oboInOwl:hasOBONamespace>GAZ</oboInOwl:hasOBONamespace>
        <oboInOwl:id>GAZ:00253655</oboInOwl:id>
        <rdfs:label>Danau Wam</rdfs:label>
    </owl:NamedIndividual>
    


    <!-- http://purl.obolibrary.org/obo/GAZ_00253656 -->

    <owl:NamedIndividual rdf:about="http://purl.obolibrary.org/obo/GAZ_00253656">
        <obo:RO_0001025 rdf:resource="http://purl.obolibrary.org/obo/GAZ_00253651"/>
        <obo:IAO_0000115>A lake. A lateral lake formed by a tributary stream being blocked through accretion by the Fly River. The lake is connected to the Fly River by a narrow channel 5 m wide. Located in the middle Fly region, upstream from the confluence of the Fly and Strickland Rivers, near Obo, Western Province.</obo:IAO_0000115>
        <oboInOwl:hasOBONamespace>GAZ</oboInOwl:hasOBONamespace>
        <oboInOwl:id>GAZ:00253656</oboInOwl:id>
        <rdfs:label>Lake Daviumbu</rdfs:label>
    </owl:NamedIndividual>
    


    <!-- http://purl.obolibrary.org/obo/GAZ_00253658 -->

    <owl:NamedIndividual rdf:about="http://purl.obolibrary.org/obo/GAZ_00253658">
        <obo:RO_0001025 rdf:resource="http://purl.obolibrary.org/obo/GAZ_00012665"/>
        <obo:IAO_0000115>A river.</obo:IAO_0000115>
        <oboInOwl:hasOBONamespace>GAZ</oboInOwl:hasOBONamespace>
        <oboInOwl:id>GAZ:00253658</oboInOwl:id>
        <rdfs:label>Bensbach River</rdfs:label>
    </owl:NamedIndividual>
    


    <!-- http://purl.obolibrary.org/obo/GAZ_00253659 -->

    <owl:NamedIndividual rdf:about="http://purl.obolibrary.org/obo/GAZ_00253659">
        <obo:RO_0001025 rdf:resource="http://purl.obolibrary.org/obo/GAZ_00012665"/>
        <obo:IAO_0000115>A protected area.</obo:IAO_0000115>
        <oboInOwl:hasOBONamespace>GAZ</oboInOwl:hasOBONamespace>
        <oboInOwl:id>GAZ:00253659</oboInOwl:id>
        <rdfs:label>Tonda Wildlife Management Area</rdfs:label>
    </owl:NamedIndividual>
    


    <!-- http://purl.obolibrary.org/obo/GAZ_00253660 -->

    <owl:NamedIndividual rdf:about="http://purl.obolibrary.org/obo/GAZ_00253660">
        <obo:RO_0001025 rdf:resource="http://purl.obolibrary.org/obo/GAZ_00012660"/>
        <obo:IAO_0000115>A freshwater crater lake. Located in the central highlands, 12 km southeast of Wabag, Enga Province.</obo:IAO_0000115>
        <oboInOwl:hasOBONamespace>GAZ</oboInOwl:hasOBONamespace>
        <oboInOwl:id>GAZ:00253660</oboInOwl:id>
        <rdfs:label>Lake Birip</rdfs:label>
    </owl:NamedIndividual>
    


    <!-- http://purl.obolibrary.org/obo/GAZ_00253661 -->

    <owl:NamedIndividual rdf:about="http://purl.obolibrary.org/obo/GAZ_00253661">
        <rdf:type rdf:resource="http://purl.obolibrary.org/obo/ENVO_00000104"/>
        <obo:RO_0001025 rdf:resource="http://purl.obolibrary.org/obo/GAZ_00012660"/>
        <obo:IAO_0000115>A basin that straddles the main watershed divide of Papua New Guinea. Lake Ipea is situated in the northern part of the basin that forms part of the Sepik River catchment. The southern part of the basin, which is some 2m higher, is part of the Fly River system.</obo:IAO_0000115>
        <oboInOwl:hasOBONamespace>GAZ</oboInOwl:hasOBONamespace>
        <oboInOwl:id>GAZ:00253661</oboInOwl:id>
        <rdfs:label>Sirunki Basin</rdfs:label>
    </owl:NamedIndividual>
    


    <!-- http://purl.obolibrary.org/obo/GAZ_00253662 -->

    <owl:NamedIndividual rdf:about="http://purl.obolibrary.org/obo/GAZ_00253662">
        <obo:RO_0001025 rdf:resource="http://purl.obolibrary.org/obo/GAZ_00253661"/>
        <obo:IAO_0000115>A lake.</obo:IAO_0000115>
        <oboInOwl:hasOBONamespace>GAZ</oboInOwl:hasOBONamespace>
        <oboInOwl:id>GAZ:00253662</oboInOwl:id>
        <rdfs:label>Lake Ipea</rdfs:label>
    </owl:NamedIndividual>
    


    <!-- http://purl.obolibrary.org/obo/GAZ_00253663 -->

    <owl:NamedIndividual rdf:about="http://purl.obolibrary.org/obo/GAZ_00253663">
        <obo:RO_0001025 rdf:resource="http://purl.obolibrary.org/obo/GAZ_00012664"/>
        <obo:IAO_0000115>A lake. Located near Mount Giluwe, 35 km east of Mendi, Southern Highlands Province. It lies between the extinct volcanic peaks of Mount Giluwe (4,367m) and Mount lalibu (3,465m). Water flows into the lake from the southern and eastern slopes of Mount Giluwe.</obo:IAO_0000115>
        <oboInOwl:hasOBONamespace>GAZ</oboInOwl:hasOBONamespace>
        <oboInOwl:id>GAZ:00253663</oboInOwl:id>
        <rdfs:label>Lake Onim</rdfs:label>
    </owl:NamedIndividual>
    


    <!-- http://purl.obolibrary.org/obo/GAZ_00253664 -->

    <owl:NamedIndividual rdf:about="http://purl.obolibrary.org/obo/GAZ_00253664">
        <rdf:type rdf:resource="http://purl.obolibrary.org/obo/ENVO_00000104"/>
        <obo:RO_0001025 rdf:resource="http://purl.obolibrary.org/obo/GAZ_00012660"/>
        <obo:IAO_0000115>A basin.</obo:IAO_0000115>
        <oboInOwl:hasOBONamespace>GAZ</oboInOwl:hasOBONamespace>
        <oboInOwl:id>GAZ:00253664</oboInOwl:id>
        <rdfs:label>Marient Basin</rdfs:label>
    </owl:NamedIndividual>
    


    <!-- http://purl.obolibrary.org/obo/GAZ_00253665 -->

    <owl:NamedIndividual rdf:about="http://purl.obolibrary.org/obo/GAZ_00253665">
        <obo:RO_0001025 rdf:resource="http://purl.obolibrary.org/obo/GAZ_00012660"/>
        <obo:IAO_0000115>A river.</obo:IAO_0000115>
        <oboInOwl:hasOBONamespace>GAZ</oboInOwl:hasOBONamespace>
        <oboInOwl:id>GAZ:00253665</oboInOwl:id>
        <rdfs:label>Marient River</rdfs:label>
    </owl:NamedIndividual>
    


    <!-- http://purl.obolibrary.org/obo/GAZ_00253666 -->

    <owl:NamedIndividual rdf:about="http://purl.obolibrary.org/obo/GAZ_00253666">
        <obo:RO_0001025 rdf:resource="http://purl.obolibrary.org/obo/GAZ_00012660"/>
        <obo:IAO_0000115>A river.</obo:IAO_0000115>
        <oboInOwl:hasOBONamespace>GAZ</oboInOwl:hasOBONamespace>
        <oboInOwl:id>GAZ:00253666</oboInOwl:id>
        <rdfs:label>Lai River</rdfs:label>
    </owl:NamedIndividual>
    


    <!-- http://purl.obolibrary.org/obo/GAZ_00253667 -->

    <owl:NamedIndividual rdf:about="http://purl.obolibrary.org/obo/GAZ_00253667">
        <obo:RO_0001025 rdf:resource="http://purl.obolibrary.org/obo/GAZ_00253664"/>
        <obo:IAO_0000115>A freshwater lake. Located in the Marient Basin, southeast of the Kandep Basin and 30 km NNE of Mendi, Enga Province. The lake is joined to the Marient River by a channel one km long.</obo:IAO_0000115>
        <oboInOwl:hasOBONamespace>GAZ</oboInOwl:hasOBONamespace>
        <oboInOwl:id>GAZ:00253667</oboInOwl:id>
        <rdfs:label>Lake Papapli</rdfs:label>
    </owl:NamedIndividual>
    


    <!-- http://purl.obolibrary.org/obo/GAZ_00253668 -->

    <owl:NamedIndividual rdf:about="http://purl.obolibrary.org/obo/GAZ_00253668">
        <obo:RO_0001025 rdf:resource="http://purl.obolibrary.org/obo/GAZ_00012660"/>
        <obo:IAO_0000115>A swampy alluvial plain fed and drained by the Lai River.</obo:IAO_0000115>
        <oboInOwl:hasOBONamespace>GAZ</oboInOwl:hasOBONamespace>
        <oboInOwl:id>GAZ:00253668</oboInOwl:id>
        <rdfs:label>Kandep Basin</rdfs:label>
    </owl:NamedIndividual>
    


    <!-- http://purl.obolibrary.org/obo/GAZ_00253669 -->

    <owl:NamedIndividual rdf:about="http://purl.obolibrary.org/obo/GAZ_00253669">
        <obo:RO_0001025 rdf:resource="http://purl.obolibrary.org/obo/GAZ_00253668"/>
        <obo:IAO_0000115>A freshwater lake. The lake is connected to the Lai River by a meandering channel approximately 10 m wide. Located in the Kandep Basin, 40 km NNW of Mendi, Enga Province.</obo:IAO_0000115>
        <oboInOwl:hasOBONamespace>GAZ</oboInOwl:hasOBONamespace>
        <oboInOwl:id>GAZ:00253669</oboInOwl:id>
        <rdfs:label>Lake Parago</rdfs:label>
    </owl:NamedIndividual>
    


    <!-- http://purl.obolibrary.org/obo/GAZ_00253670 -->

    <owl:NamedIndividual rdf:about="http://purl.obolibrary.org/obo/GAZ_00253670">
        <obo:RO_0001025 rdf:resource="http://purl.obolibrary.org/obo/GAZ_00012664"/>
        <obo:IAO_0000115>A freshwater lake. Located 5 km west of Tan, Southern Highlands Province.</obo:IAO_0000115>
        <oboInOwl:hasOBONamespace>GAZ</oboInOwl:hasOBONamespace>
        <oboInOwl:id>GAZ:00253670</oboInOwl:id>
        <rdfs:label>Lake Wololo</rdfs:label>
    </owl:NamedIndividual>
    


    <!-- http://purl.obolibrary.org/obo/GAZ_00253671 -->

    <owl:NamedIndividual rdf:about="http://purl.obolibrary.org/obo/GAZ_00253671">
        <obo:RO_0001025 rdf:resource="http://purl.obolibrary.org/obo/GAZ_00012664"/>
        <obo:IAO_0000115>A small lake situated in a sinkhole. Located 14 km WNW of Tan, Southern Highlands Province.</obo:IAO_0000115>
        <oboInOwl:hasOBONamespace>GAZ</oboInOwl:hasOBONamespace>
        <oboInOwl:id>GAZ:00253671</oboInOwl:id>
        <rdfs:label>Lake Wongabi</rdfs:label>
    </owl:NamedIndividual>
    


    <!-- http://purl.obolibrary.org/obo/GAZ_00253672 -->

    <owl:NamedIndividual rdf:about="http://purl.obolibrary.org/obo/GAZ_00253672">
        <obo:RO_0001025 rdf:resource="http://purl.obolibrary.org/obo/GAZ_00012664"/>
        <obo:IAO_0000115>A freshwater lake. Located near Kopiago, 70 km northwest of Tan, Southern Highlands Province.</obo:IAO_0000115>
        <oboInOwl:hasOBONamespace>GAZ</oboInOwl:hasOBONamespace>
        <oboInOwl:id>GAZ:00253672</oboInOwl:id>
        <rdfs:label>Lake Kopiago</rdfs:label>
    </owl:NamedIndividual>
    


    <!-- http://purl.obolibrary.org/obo/GAZ_00253673 -->

    <owl:NamedIndividual rdf:about="http://purl.obolibrary.org/obo/GAZ_00253673">
        <obo:RO_0001025 rdf:resource="http://purl.obolibrary.org/obo/GAZ_00016819"/>
        <obo:IAO_0000115>A wetland. Located on the southwest coast, on the shores of Malai Bay, of Manus Island, Manus Province.</obo:IAO_0000115>
        <oboInOwl:hasOBONamespace>GAZ</oboInOwl:hasOBONamespace>
        <oboInOwl:id>GAZ:00253673</oboInOwl:id>
        <rdfs:label>Malai Wetland</rdfs:label>
    </owl:NamedIndividual>
    


    <!-- http://purl.obolibrary.org/obo/GAZ_00253674 -->

    <owl:NamedIndividual rdf:about="http://purl.obolibrary.org/obo/GAZ_00253674">
        <obo:RO_0001025 rdf:resource="http://purl.obolibrary.org/obo/GAZ_00016819"/>
        <obo:IAO_0000115>A wetland. Located near Kelaua Harbour on the southeast coast of Manus Island, Manus Province.</obo:IAO_0000115>
        <oboInOwl:hasOBONamespace>GAZ</oboInOwl:hasOBONamespace>
        <oboInOwl:id>GAZ:00253674</oboInOwl:id>
        <rdfs:label>Kelaua Wetland</rdfs:label>
    </owl:NamedIndividual>
    


    <!-- http://purl.obolibrary.org/obo/GAZ_00253675 -->

    <owl:NamedIndividual rdf:about="http://purl.obolibrary.org/obo/GAZ_00253675">
        <obo:RO_0001025 rdf:resource="http://purl.obolibrary.org/obo/GAZ_00007179"/>
        <obo:IAO_0000115>One of the Admiralty Islands.</obo:IAO_0000115>
        <oboInOwl:hasOBONamespace>GAZ</oboInOwl:hasOBONamespace>
        <oboInOwl:id>GAZ:00253675</oboInOwl:id>
        <rdfs:label>Patuam Island</rdfs:label>
    </owl:NamedIndividual>
    


    <!-- http://purl.obolibrary.org/obo/GAZ_00253676 -->

    <owl:NamedIndividual rdf:about="http://purl.obolibrary.org/obo/GAZ_00253676">
        <obo:RO_0001025 rdf:resource="http://purl.obolibrary.org/obo/GAZ_00007179"/>
        <obo:IAO_0000115>An island located off the west coast of the main island of Manus in the Admiralty Group.</obo:IAO_0000115>
        <oboInOwl:hasOBONamespace>GAZ</oboInOwl:hasOBONamespace>
        <oboInOwl:id>GAZ:00253676</oboInOwl:id>
        <rdfs:label>Bipi Island</rdfs:label>
    </owl:NamedIndividual>
    


    <!-- http://purl.obolibrary.org/obo/GAZ_00253677 -->

    <owl:NamedIndividual rdf:about="http://purl.obolibrary.org/obo/GAZ_00253677">
        <obo:RO_0001025 rdf:resource="http://purl.obolibrary.org/obo/GAZ_00016819"/>
        <obo:IAO_0000115>A harbor. Located on Manus Island, Admiralty Islands.</obo:IAO_0000115>
        <oboInOwl:hasOBONamespace>GAZ</oboInOwl:hasOBONamespace>
        <oboInOwl:id>GAZ:00253677</oboInOwl:id>
        <rdfs:label>Seeadler Harbor</rdfs:label>
    </owl:NamedIndividual>
    


    <!-- http://purl.obolibrary.org/obo/GAZ_00253678 -->

    <owl:NamedIndividual rdf:about="http://purl.obolibrary.org/obo/GAZ_00253678">
        <obo:RO_0001025 rdf:resource="http://purl.obolibrary.org/obo/GAZ_00005189"/>
        <obo:RO_0001025 rdf:resource="http://purl.obolibrary.org/obo/GAZ_00005191"/>
        <obo:IAO_0000115>A wetland. A large area of riverine marshes and floodplains with herbaceous swamps and oxbow lakes, to the south of three bays, Riebeck, Eleonora and Emeline, on the northwest coast of West New Britain. The floodplains are drained by several rivers including the Kulu (emptying into Riebeck Bay), the Kapuluk (Eleonora Bay) and Via (Emeline Bay). Located 10-70 km west of Kimbe, on the north coast of West New Britain Province, New Britain.</obo:IAO_0000115>
        <oboInOwl:hasOBONamespace>GAZ</oboInOwl:hasOBONamespace>
        <oboInOwl:id>GAZ:00253678</oboInOwl:id>
        <rdfs:label>Namo Wetland</rdfs:label>
    </owl:NamedIndividual>
    


    <!-- http://purl.obolibrary.org/obo/GAZ_00253679 -->

    <owl:NamedIndividual rdf:about="http://purl.obolibrary.org/obo/GAZ_00253679">
        <obo:RO_0001025 rdf:resource="http://purl.obolibrary.org/obo/GAZ_00253678"/>
        <obo:IAO_0000115>A freshwater lake.</obo:IAO_0000115>
        <oboInOwl:hasOBONamespace>GAZ</oboInOwl:hasOBONamespace>
        <oboInOwl:id>GAZ:00253679</oboInOwl:id>
        <rdfs:label>Lake Namo</rdfs:label>
    </owl:NamedIndividual>
    


    <!-- http://purl.obolibrary.org/obo/GAZ_00253680 -->

    <owl:NamedIndividual rdf:about="http://purl.obolibrary.org/obo/GAZ_00253680">
        <obo:RO_0001025 rdf:resource="http://purl.obolibrary.org/obo/GAZ_00005189"/>
        <obo:RO_0001025 rdf:resource="http://purl.obolibrary.org/obo/GAZ_00005191"/>
        <obo:IAO_0000115>A river.</obo:IAO_0000115>
        <oboInOwl:hasOBONamespace>GAZ</oboInOwl:hasOBONamespace>
        <oboInOwl:id>GAZ:00253680</oboInOwl:id>
        <rdfs:label>Kulu River</rdfs:label>
    </owl:NamedIndividual>
    


    <!-- http://purl.obolibrary.org/obo/GAZ_00253681 -->

    <owl:NamedIndividual rdf:about="http://purl.obolibrary.org/obo/GAZ_00253681">
        <obo:RO_0001025 rdf:resource="http://purl.obolibrary.org/obo/GAZ_00005189"/>
        <obo:RO_0001025 rdf:resource="http://purl.obolibrary.org/obo/GAZ_00005191"/>
        <obo:IAO_0000115>A river.</obo:IAO_0000115>
        <oboInOwl:hasOBONamespace>GAZ</oboInOwl:hasOBONamespace>
        <oboInOwl:id>GAZ:00253681</oboInOwl:id>
        <rdfs:label>Kapuluk River</rdfs:label>
    </owl:NamedIndividual>
    


    <!-- http://purl.obolibrary.org/obo/GAZ_00253682 -->

    <owl:NamedIndividual rdf:about="http://purl.obolibrary.org/obo/GAZ_00253682">
        <obo:RO_0001025 rdf:resource="http://purl.obolibrary.org/obo/GAZ_00005189"/>
        <obo:RO_0001025 rdf:resource="http://purl.obolibrary.org/obo/GAZ_00005191"/>
        <obo:IAO_0000115>A river.</obo:IAO_0000115>
        <oboInOwl:hasOBONamespace>GAZ</oboInOwl:hasOBONamespace>
        <oboInOwl:id>GAZ:00253682</oboInOwl:id>
        <rdfs:label>Via River</rdfs:label>
    </owl:NamedIndividual>
    


    <!-- http://purl.obolibrary.org/obo/GAZ_00253683 -->

    <owl:NamedIndividual rdf:about="http://purl.obolibrary.org/obo/GAZ_00253683">
        <obo:RO_0001025 rdf:resource="http://purl.obolibrary.org/obo/GAZ_00005189"/>
        <obo:RO_0001025 rdf:resource="http://purl.obolibrary.org/obo/GAZ_00005191"/>
        <obo:IAO_0000115>A bay. Located on the N coast of New Britain.</obo:IAO_0000115>
        <oboInOwl:hasOBONamespace>GAZ</oboInOwl:hasOBONamespace>
        <oboInOwl:id>GAZ:00253683</oboInOwl:id>
        <rdfs:label>Riebeck Bay</rdfs:label>
    </owl:NamedIndividual>
    


    <!-- http://purl.obolibrary.org/obo/GAZ_00253684 -->

    <owl:NamedIndividual rdf:about="http://purl.obolibrary.org/obo/GAZ_00253684">
        <obo:RO_0001025 rdf:resource="http://purl.obolibrary.org/obo/GAZ_00005189"/>
        <obo:RO_0001025 rdf:resource="http://purl.obolibrary.org/obo/GAZ_00005191"/>
        <obo:IAO_0000115>A bay. Located on the N coast of New Britain.</obo:IAO_0000115>
        <oboInOwl:hasOBONamespace>GAZ</oboInOwl:hasOBONamespace>
        <oboInOwl:id>GAZ:00253684</oboInOwl:id>
        <rdfs:label>Eleonora Bay</rdfs:label>
    </owl:NamedIndividual>
    


    <!-- http://purl.obolibrary.org/obo/GAZ_00253685 -->

    <owl:NamedIndividual rdf:about="http://purl.obolibrary.org/obo/GAZ_00253685">
        <obo:RO_0001025 rdf:resource="http://purl.obolibrary.org/obo/GAZ_00005189"/>
        <obo:RO_0001025 rdf:resource="http://purl.obolibrary.org/obo/GAZ_00005191"/>
        <obo:IAO_0000115>A bay. Located on the N coast of New Britain.</obo:IAO_0000115>
        <oboInOwl:hasOBONamespace>GAZ</oboInOwl:hasOBONamespace>
        <oboInOwl:id>GAZ:00253685</oboInOwl:id>
        <rdfs:label>Emeline Bay</rdfs:label>
    </owl:NamedIndividual>
    


    <!-- http://purl.obolibrary.org/obo/GAZ_00253686 -->

    <owl:NamedIndividual rdf:about="http://purl.obolibrary.org/obo/GAZ_00253686">
        <obo:RO_0001025 rdf:resource="http://purl.obolibrary.org/obo/GAZ_00053908"/>
        <obo:IAO_0000115>A caldera lake.</obo:IAO_0000115>
        <oboInOwl:hasOBONamespace>GAZ</oboInOwl:hasOBONamespace>
        <oboInOwl:id>GAZ:00253686</oboInOwl:id>
        <rdfs:label>Lake Dakataua</rdfs:label>
    </owl:NamedIndividual>
    


    <!-- http://purl.obolibrary.org/obo/GAZ_00253687 -->

    <owl:NamedIndividual rdf:about="http://purl.obolibrary.org/obo/GAZ_00253687">
        <obo:RO_0001025 rdf:resource="http://purl.obolibrary.org/obo/GAZ_00053915"/>
        <obo:IAO_0000115>A freshwater caldera lake.</obo:IAO_0000115>
        <oboInOwl:hasOBONamespace>GAZ</oboInOwl:hasOBONamespace>
        <oboInOwl:id>GAZ:00253687</oboInOwl:id>
        <rdfs:label>Lake Hargy</rdfs:label>
    </owl:NamedIndividual>
    


    <!-- http://purl.obolibrary.org/obo/GAZ_00253688 -->

    <owl:NamedIndividual rdf:about="http://purl.obolibrary.org/obo/GAZ_00253688">
        <rdf:type rdf:resource="http://purl.obolibrary.org/obo/ENVO_00000305"/>
        <obo:RO_0001025 rdf:resource="http://purl.obolibrary.org/obo/GAZ_00005189"/>
        <obo:RO_0001025 rdf:resource="http://purl.obolibrary.org/obo/GAZ_00005191"/>
        <obo:IAO_0000115>A cape.</obo:IAO_0000115>
        <oboInOwl:hasOBONamespace>GAZ</oboInOwl:hasOBONamespace>
        <oboInOwl:id>GAZ:00253688</oboInOwl:id>
        <rdfs:label>Cape Hoskins</rdfs:label>
    </owl:NamedIndividual>
    


    <!-- http://purl.obolibrary.org/obo/GAZ_00253689 -->

    <owl:NamedIndividual rdf:about="http://purl.obolibrary.org/obo/GAZ_00253689">
        <obo:RO_0001025 rdf:resource="http://purl.obolibrary.org/obo/GAZ_00118076"/>
        <obo:IAO_0000115>A populated place. The capital of East New Britain in Papua New Guinea. The capital was moved from Rabaul in 1994 when the volcanoes Tavurvur and Vulcan erupted.</obo:IAO_0000115>
        <oboInOwl:hasOBONamespace>GAZ</oboInOwl:hasOBONamespace>
        <oboInOwl:id>GAZ:00253689</oboInOwl:id>
        <rdfs:label>Kokopo</rdfs:label>
    </owl:NamedIndividual>
    


    <!-- http://purl.obolibrary.org/obo/GAZ_00253690 -->

    <owl:NamedIndividual rdf:about="http://purl.obolibrary.org/obo/GAZ_00253690">
        <obo:RO_0001025 rdf:resource="http://purl.obolibrary.org/obo/GAZ_00005189"/>
        <obo:RO_0001025 rdf:resource="http://purl.obolibrary.org/obo/GAZ_00005192"/>
        <obo:IAO_0000115>A wetland. A large area of estuarine marshes and floodplains along the lower courses of the Toriu, Nesai and Pali Rivers and several smaller rivers, draining into a large bay on the northeast coast of New Britain. Located on the northeast coast of New Britain, 80 km southwest of Rabaul, East New Britain Province.</obo:IAO_0000115>
        <oboInOwl:hasOBONamespace>GAZ</oboInOwl:hasOBONamespace>
        <oboInOwl:id>GAZ:00253690</oboInOwl:id>
        <rdfs:label>Toriu Wetland</rdfs:label>
    </owl:NamedIndividual>
    


    <!-- http://purl.obolibrary.org/obo/GAZ_00253691 -->

    <owl:NamedIndividual rdf:about="http://purl.obolibrary.org/obo/GAZ_00253691">
        <obo:RO_0001025 rdf:resource="http://purl.obolibrary.org/obo/GAZ_00005192"/>
        <obo:IAO_0000115>A river.</obo:IAO_0000115>
        <oboInOwl:hasOBONamespace>GAZ</oboInOwl:hasOBONamespace>
        <oboInOwl:id>GAZ:00253691</oboInOwl:id>
        <rdfs:label>Toriu, River</rdfs:label>
    </owl:NamedIndividual>
    


    <!-- http://purl.obolibrary.org/obo/GAZ_00253692 -->

    <owl:NamedIndividual rdf:about="http://purl.obolibrary.org/obo/GAZ_00253692">
        <obo:RO_0001025 rdf:resource="http://purl.obolibrary.org/obo/GAZ_00005192"/>
        <obo:IAO_0000115>A river.</obo:IAO_0000115>
        <oboInOwl:hasOBONamespace>GAZ</oboInOwl:hasOBONamespace>
        <oboInOwl:id>GAZ:00253692</oboInOwl:id>
        <rdfs:label>Nesai River</rdfs:label>
    </owl:NamedIndividual>
    


    <!-- http://purl.obolibrary.org/obo/GAZ_00253693 -->

    <owl:NamedIndividual rdf:about="http://purl.obolibrary.org/obo/GAZ_00253693">
        <obo:RO_0001025 rdf:resource="http://purl.obolibrary.org/obo/GAZ_00005192"/>
        <obo:IAO_0000115>A river.</obo:IAO_0000115>
        <oboInOwl:hasOBONamespace>GAZ</oboInOwl:hasOBONamespace>
        <oboInOwl:id>GAZ:00253693</oboInOwl:id>
        <rdfs:label>Pali River</rdfs:label>
    </owl:NamedIndividual>
    


    <!-- http://purl.obolibrary.org/obo/GAZ_00253694 -->

    <owl:NamedIndividual rdf:about="http://purl.obolibrary.org/obo/GAZ_00253694">
        <obo:RO_0001025 rdf:resource="http://purl.obolibrary.org/obo/GAZ_00005184"/>
        <obo:IAO_0000115>A wetland. Located between Laruma Point and Motupena Point, on the west coast of Bougainville Island, North Solomon Islands.</obo:IAO_0000115>
        <oboInOwl:hasOBONamespace>GAZ</oboInOwl:hasOBONamespace>
        <oboInOwl:id>GAZ:00253694</oboInOwl:id>
        <rdfs:label>Empress Augusta Bay Wetland</rdfs:label>
    </owl:NamedIndividual>
    


    <!-- http://purl.obolibrary.org/obo/GAZ_00253695 -->

    <owl:NamedIndividual rdf:about="http://purl.obolibrary.org/obo/GAZ_00253695">
        <obo:RO_0001025 rdf:resource="http://purl.obolibrary.org/obo/GAZ_00005184"/>
        <obo:IAO_0000115>A river.</obo:IAO_0000115>
        <oboInOwl:hasOBONamespace>GAZ</oboInOwl:hasOBONamespace>
        <oboInOwl:id>GAZ:00253695</oboInOwl:id>
        <rdfs:label>Laruma River</rdfs:label>
    </owl:NamedIndividual>
    


    <!-- http://purl.obolibrary.org/obo/GAZ_00253696 -->

    <owl:NamedIndividual rdf:about="http://purl.obolibrary.org/obo/GAZ_00253696">
        <obo:RO_0001025 rdf:resource="http://purl.obolibrary.org/obo/GAZ_00005184"/>
        <obo:IAO_0000115>A river.</obo:IAO_0000115>
        <oboInOwl:hasOBONamespace>GAZ</oboInOwl:hasOBONamespace>
        <oboInOwl:id>GAZ:00253696</oboInOwl:id>
        <rdfs:label>Torokina River</rdfs:label>
    </owl:NamedIndividual>
    


    <!-- http://purl.obolibrary.org/obo/GAZ_00253697 -->

    <owl:NamedIndividual rdf:about="http://purl.obolibrary.org/obo/GAZ_00253697">
        <obo:RO_0001025 rdf:resource="http://purl.obolibrary.org/obo/GAZ_00005184"/>
        <obo:IAO_0000115>A river.</obo:IAO_0000115>
        <oboInOwl:hasOBONamespace>GAZ</oboInOwl:hasOBONamespace>
        <oboInOwl:id>GAZ:00253697</oboInOwl:id>
        <rdfs:label>Jaba River</rdfs:label>
    </owl:NamedIndividual>
    


    <!-- http://purl.obolibrary.org/obo/GAZ_00253698 -->

    <owl:NamedIndividual rdf:about="http://purl.obolibrary.org/obo/GAZ_00253698">
        <obo:RO_0001025 rdf:resource="http://purl.obolibrary.org/obo/GAZ_00005184"/>
        <obo:IAO_0000115>A river.</obo:IAO_0000115>
        <oboInOwl:hasOBONamespace>GAZ</oboInOwl:hasOBONamespace>
        <oboInOwl:id>GAZ:00253698</oboInOwl:id>
        <rdfs:label>Pagana River</rdfs:label>
    </owl:NamedIndividual>
    


    <!-- http://purl.obolibrary.org/obo/GAZ_00253699 -->

    <owl:NamedIndividual rdf:about="http://purl.obolibrary.org/obo/GAZ_00253699">
        <obo:RO_0001025 rdf:resource="http://purl.obolibrary.org/obo/GAZ_00005184"/>
        <obo:IAO_0000115>A river.</obo:IAO_0000115>
        <oboInOwl:hasOBONamespace>GAZ</oboInOwl:hasOBONamespace>
        <oboInOwl:id>GAZ:00253699</oboInOwl:id>
        <rdfs:label>Hupai River</rdfs:label>
    </owl:NamedIndividual>
    


    <!-- http://purl.obolibrary.org/obo/GAZ_00253700 -->

    <owl:NamedIndividual rdf:about="http://purl.obolibrary.org/obo/GAZ_00253700">
        <obo:RO_0001025 rdf:resource="http://purl.obolibrary.org/obo/GAZ_00005184"/>
        <obo:IAO_0000115>A wetland. Located on the southeast coast or Bougainville Island, in the North Solomon Islands.</obo:IAO_0000115>
        <oboInOwl:hasOBONamespace>GAZ</oboInOwl:hasOBONamespace>
        <oboInOwl:id>GAZ:00253700</oboInOwl:id>
        <rdfs:label>Abia Wetland</rdfs:label>
    </owl:NamedIndividual>
    


    <!-- http://purl.obolibrary.org/obo/GAZ_00253701 -->

    <owl:NamedIndividual rdf:about="http://purl.obolibrary.org/obo/GAZ_00253701">
        <obo:RO_0001025 rdf:resource="http://purl.obolibrary.org/obo/GAZ_00253700"/>
        <obo:IAO_0000115>A freshwater lake.</obo:IAO_0000115>
        <oboInOwl:hasOBONamespace>GAZ</oboInOwl:hasOBONamespace>
        <oboInOwl:id>GAZ:00253701</oboInOwl:id>
        <rdfs:label>Lake Lehala</rdfs:label>
    </owl:NamedIndividual>
    


    <!-- http://purl.obolibrary.org/obo/GAZ_00253703 -->

    <owl:NamedIndividual rdf:about="http://purl.obolibrary.org/obo/GAZ_00253703">
        <obo:RO_0001025 rdf:resource="http://purl.obolibrary.org/obo/GAZ_00005184"/>
        <oboInOwl:hasOBONamespace>GAZ</oboInOwl:hasOBONamespace>
        <oboInOwl:id>GAZ:00253703</oboInOwl:id>
        <rdfs:label>Abia River</rdfs:label>
    </owl:NamedIndividual>
    


    <!-- http://purl.obolibrary.org/obo/GAZ_00253704 -->

    <owl:NamedIndividual rdf:about="http://purl.obolibrary.org/obo/GAZ_00253704">
        <obo:RO_0001025 rdf:resource="http://purl.obolibrary.org/obo/GAZ_00005184"/>
        <obo:IAO_0000115>A marine protected area.</obo:IAO_0000115>
        <oboInOwl:hasOBONamespace>GAZ</oboInOwl:hasOBONamespace>
        <oboInOwl:id>GAZ:00253704</oboInOwl:id>
        <rdfs:label>Pirung Wildlife Management Area</rdfs:label>
    </owl:NamedIndividual>
    


    <!-- http://purl.obolibrary.org/obo/GAZ_00253791 -->

    <owl:NamedIndividual rdf:about="http://purl.obolibrary.org/obo/GAZ_00253791">
        <obo:RO_0001025 rdf:resource="http://purl.obolibrary.org/obo/GAZ_00012665"/>
        <obo:IAO_0000115>A marine protected area that starts from the Binaturi river on the West, to Moon Passage in Warrior Reef complex in the south then East on Parama island.</obo:IAO_0000115>
        <oboInOwl:hasOBONamespace>GAZ</oboInOwl:hasOBONamespace>
        <oboInOwl:id>GAZ:00253791</oboInOwl:id>
        <rdfs:label>Maza Wildlife Management Area</rdfs:label>
    </owl:NamedIndividual>
    


    <!-- http://purl.obolibrary.org/obo/GAZ_00253792 -->

    <owl:NamedIndividual rdf:about="http://purl.obolibrary.org/obo/GAZ_00253792">
        <obo:RO_0001025 rdf:resource="http://purl.obolibrary.org/obo/GAZ_00253791"/>
        <obo:IAO_0000115>A coral reef.</obo:IAO_0000115>
        <oboInOwl:hasOBONamespace>GAZ</oboInOwl:hasOBONamespace>
        <oboInOwl:id>GAZ:00253792</oboInOwl:id>
        <rdfs:label>Wapa Reef</rdfs:label>
    </owl:NamedIndividual>
    


    <!-- http://purl.obolibrary.org/obo/GAZ_00253793 -->

    <owl:NamedIndividual rdf:about="http://purl.obolibrary.org/obo/GAZ_00253793">
        <obo:RO_0001025 rdf:resource="http://purl.obolibrary.org/obo/GAZ_00253791"/>
        <obo:IAO_0000115>A coral reef.</obo:IAO_0000115>
        <oboInOwl:hasOBONamespace>GAZ</oboInOwl:hasOBONamespace>
        <oboInOwl:id>GAZ:00253793</oboInOwl:id>
        <rdfs:label>Auomaza Reef</rdfs:label>
    </owl:NamedIndividual>
    


    <!-- http://purl.obolibrary.org/obo/GAZ_00253794 -->

    <owl:NamedIndividual rdf:about="http://purl.obolibrary.org/obo/GAZ_00253794">
        <obo:RO_0001025 rdf:resource="http://purl.obolibrary.org/obo/GAZ_00253791"/>
        <obo:IAO_0000115>A coral reefs.</obo:IAO_0000115>
        <oboInOwl:hasOBONamespace>GAZ</oboInOwl:hasOBONamespace>
        <oboInOwl:id>GAZ:00253794</oboInOwl:id>
        <rdfs:label>Gemini Reefs</rdfs:label>
    </owl:NamedIndividual>
    


    <!-- http://purl.obolibrary.org/obo/GAZ_00253795 -->

    <owl:NamedIndividual rdf:about="http://purl.obolibrary.org/obo/GAZ_00253795">
        <obo:RO_0001025 rdf:resource="http://purl.obolibrary.org/obo/GAZ_00253791"/>
        <obo:IAO_0000115>A coral reefs.</obo:IAO_0000115>
        <oboInOwl:hasOBONamespace>GAZ</oboInOwl:hasOBONamespace>
        <oboInOwl:id>GAZ:00253795</oboInOwl:id>
        <rdfs:label>Silver Reefs</rdfs:label>
    </owl:NamedIndividual>
    


    <!-- http://purl.obolibrary.org/obo/GAZ_00253796 -->

    <owl:NamedIndividual rdf:about="http://purl.obolibrary.org/obo/GAZ_00253796">
        <obo:RO_0001025 rdf:resource="http://purl.obolibrary.org/obo/GAZ_00253791"/>
        <obo:IAO_0000115>A coral reefs.</obo:IAO_0000115>
        <oboInOwl:hasOBONamespace>GAZ</oboInOwl:hasOBONamespace>
        <oboInOwl:id>GAZ:00253796</oboInOwl:id>
        <rdfs:label>Kokopi Reefs</rdfs:label>
    </owl:NamedIndividual>
    


    <!-- http://purl.obolibrary.org/obo/GAZ_00253797 -->

    <owl:NamedIndividual rdf:about="http://purl.obolibrary.org/obo/GAZ_00253797">
        <obo:RO_0001025 rdf:resource="http://purl.obolibrary.org/obo/GAZ_00253791"/>
        <obo:IAO_0000115>A coral reefs.</obo:IAO_0000115>
        <oboInOwl:hasOBONamespace>GAZ</oboInOwl:hasOBONamespace>
        <oboInOwl:id>GAZ:00253797</oboInOwl:id>
        <rdfs:label>Parakivori Reefs</rdfs:label>
    </owl:NamedIndividual>
    


    <!-- http://purl.obolibrary.org/obo/GAZ_00253798 -->

    <owl:NamedIndividual rdf:about="http://purl.obolibrary.org/obo/GAZ_00253798">
        <obo:RO_0001025 rdf:resource="http://purl.obolibrary.org/obo/GAZ_00253791"/>
        <obo:IAO_0000115>A coral reefs.</obo:IAO_0000115>
        <oboInOwl:hasOBONamespace>GAZ</oboInOwl:hasOBONamespace>
        <oboInOwl:id>GAZ:00253798</oboInOwl:id>
        <rdfs:label>Kumusi Reefs</rdfs:label>
    </owl:NamedIndividual>
    


    <!-- http://purl.obolibrary.org/obo/GAZ_00253799 -->

    <owl:NamedIndividual rdf:about="http://purl.obolibrary.org/obo/GAZ_00253799">
        <obo:RO_0001025 rdf:resource="http://purl.obolibrary.org/obo/GAZ_00253791"/>
        <obo:IAO_0000115>A coral reefs.</obo:IAO_0000115>
        <oboInOwl:hasOBONamespace>GAZ</oboInOwl:hasOBONamespace>
        <oboInOwl:id>GAZ:00253799</oboInOwl:id>
        <rdfs:label>Otamabu Reefs</rdfs:label>
    </owl:NamedIndividual>
    


    <!-- http://purl.obolibrary.org/obo/GAZ_00253800 -->

    <owl:NamedIndividual rdf:about="http://purl.obolibrary.org/obo/GAZ_00253800">
        <obo:RO_0001025 rdf:resource="http://purl.obolibrary.org/obo/GAZ_00253791"/>
        <obo:IAO_0000115>An island.</obo:IAO_0000115>
        <oboInOwl:hasOBONamespace>GAZ</oboInOwl:hasOBONamespace>
        <oboInOwl:id>GAZ:00253800</oboInOwl:id>
        <rdfs:label>Bistrow Island</rdfs:label>
    </owl:NamedIndividual>
    


    <!-- http://purl.obolibrary.org/obo/GAZ_00253801 -->

    <owl:NamedIndividual rdf:about="http://purl.obolibrary.org/obo/GAZ_00253801">
        <obo:RO_0001025 rdf:resource="http://purl.obolibrary.org/obo/GAZ_00253791"/>
        <obo:IAO_0000115>An island.</obo:IAO_0000115>
        <oboInOwl:hasOBONamespace>GAZ</oboInOwl:hasOBONamespace>
        <oboInOwl:id>GAZ:00253801</oboInOwl:id>
        <rdfs:label>Daru Island</rdfs:label>
    </owl:NamedIndividual>
    


    <!-- http://purl.obolibrary.org/obo/GAZ_00253802 -->

    <owl:NamedIndividual rdf:about="http://purl.obolibrary.org/obo/GAZ_00253802">
        <obo:RO_0001025 rdf:resource="http://purl.obolibrary.org/obo/GAZ_00146248"/>
        <obo:IAO_0000115>Coral reefs.</obo:IAO_0000115>
        <oboInOwl:hasOBONamespace>GAZ</oboInOwl:hasOBONamespace>
        <oboInOwl:id>GAZ:00253802</oboInOwl:id>
        <rdfs:label>Eastern Fields</rdfs:label>
    </owl:NamedIndividual>
    


    <!-- http://purl.obolibrary.org/obo/GAZ_00253803 -->

    <owl:NamedIndividual rdf:about="http://purl.obolibrary.org/obo/GAZ_00253803">
        <obo:RO_0001025 rdf:resource="http://purl.obolibrary.org/obo/GAZ_00012657"/>
        <obo:IAO_0000115>An island. Located S of Bootless Inlet.</obo:IAO_0000115>
        <oboInOwl:hasOBONamespace>GAZ</oboInOwl:hasOBONamespace>
        <oboInOwl:id>GAZ:00253803</oboInOwl:id>
        <rdfs:label>Motupore Island</rdfs:label>
    </owl:NamedIndividual>
    


    <!-- http://purl.obolibrary.org/obo/GAZ_00253804 -->

    <owl:NamedIndividual rdf:about="http://purl.obolibrary.org/obo/GAZ_00253804">
        <obo:RO_0001025 rdf:resource="http://purl.obolibrary.org/obo/GAZ_00012657"/>
        <obo:IAO_0000115>A marine protected area. Established 1981-01-01.</obo:IAO_0000115>
        <oboInOwl:hasOBONamespace>GAZ</oboInOwl:hasOBONamespace>
        <oboInOwl:id>GAZ:00253804</oboInOwl:id>
        <rdfs:label>Horseshoe Reed Marine Park</rdfs:label>
    </owl:NamedIndividual>
    


    <!-- http://purl.obolibrary.org/obo/GAZ_00253805 -->

    <owl:NamedIndividual rdf:about="http://purl.obolibrary.org/obo/GAZ_00253805">
        <rdf:type rdf:resource="http://purl.obolibrary.org/obo/ENVO_00000130"/>
        <obo:IAO_0000115>A barrier reef along the coast SE of Port Moresby.</obo:IAO_0000115>
        <oboInOwl:hasOBONamespace>GAZ</oboInOwl:hasOBONamespace>
        <oboInOwl:id>GAZ:00253805</oboInOwl:id>
        <rdfs:label>Papuan Barrier Reef</rdfs:label>
    </owl:NamedIndividual>
    


    <!-- http://purl.obolibrary.org/obo/GAZ_00253806 -->

    <owl:NamedIndividual rdf:about="http://purl.obolibrary.org/obo/GAZ_00253806">
        <obo:RO_0001025 rdf:resource="http://purl.obolibrary.org/obo/GAZ_00012666"/>
        <obo:IAO_0000115>An island.</obo:IAO_0000115>
        <oboInOwl:hasOBONamespace>GAZ</oboInOwl:hasOBONamespace>
        <oboInOwl:id>GAZ:00253806</oboInOwl:id>
        <rdfs:label>Baniara Island</rdfs:label>
    </owl:NamedIndividual>
    


    <!-- http://purl.obolibrary.org/obo/GAZ_00253807 -->

    <owl:NamedIndividual rdf:about="http://purl.obolibrary.org/obo/GAZ_00253807">
        <obo:RO_0001025 rdf:resource="http://purl.obolibrary.org/obo/GAZ_00253806"/>
        <obo:IAO_0000115>A protected area. Established 1975-01-01.</obo:IAO_0000115>
        <oboInOwl:hasOBONamespace>GAZ</oboInOwl:hasOBONamespace>
        <oboInOwl:id>GAZ:00253807</oboInOwl:id>
        <rdfs:label>Baniara Island Fauna Protected Area</rdfs:label>
    </owl:NamedIndividual>
    


    <!-- http://purl.obolibrary.org/obo/GAZ_00253808 -->

    <owl:NamedIndividual rdf:about="http://purl.obolibrary.org/obo/GAZ_00253808">
        <obo:RO_0001025 rdf:resource="http://purl.obolibrary.org/obo/GAZ_00007182"/>
        <obo:IAO_0000115>Islands. Located 81 km southeast from Normanby Island (in the D&apos;Entrecasteaux Islands group) and 35 km directly north form the Louisiade Archipelago&apos;s Long Reef. The group forms a pear-shaped reef formation of 9 km by 21 km, enclosing a central lagoon of up to 30 m in depth.</obo:IAO_0000115>
        <oboInOwl:hasOBONamespace>GAZ</oboInOwl:hasOBONamespace>
        <oboInOwl:id>GAZ:00253808</oboInOwl:id>
        <rdfs:label>Conflict Group</rdfs:label>
    </owl:NamedIndividual>
    


    <!-- http://purl.obolibrary.org/obo/GAZ_00253809 -->

    <owl:NamedIndividual rdf:about="http://purl.obolibrary.org/obo/GAZ_00253809">
        <obo:RO_0001025 rdf:resource="http://purl.obolibrary.org/obo/GAZ_00253808"/>
        <obo:IAO_0000115>An island in the Conflict Group.</obo:IAO_0000115>
        <oboInOwl:hasOBONamespace>GAZ</oboInOwl:hasOBONamespace>
        <oboInOwl:id>GAZ:00253809</oboInOwl:id>
        <rdfs:label>Ilai Island</rdfs:label>
    </owl:NamedIndividual>
    


    <!-- http://purl.obolibrary.org/obo/GAZ_00253810 -->

    <owl:NamedIndividual rdf:about="http://purl.obolibrary.org/obo/GAZ_00253810">
        <obo:RO_0001025 rdf:resource="http://purl.obolibrary.org/obo/GAZ_00253808"/>
        <obo:IAO_0000115>An island in the Conflict Group.</obo:IAO_0000115>
        <oboInOwl:hasOBONamespace>GAZ</oboInOwl:hasOBONamespace>
        <oboInOwl:id>GAZ:00253810</oboInOwl:id>
        <rdfs:label>Panasesa Island</rdfs:label>
    </owl:NamedIndividual>
    


    <!-- http://purl.obolibrary.org/obo/GAZ_00253811 -->

    <owl:NamedIndividual rdf:about="http://purl.obolibrary.org/obo/GAZ_00253811">
        <obo:RO_0001025 rdf:resource="http://purl.obolibrary.org/obo/GAZ_00253808"/>
        <obo:IAO_0000115>An island in the Conflict Group.</obo:IAO_0000115>
        <oboInOwl:hasOBONamespace>GAZ</oboInOwl:hasOBONamespace>
        <oboInOwl:id>GAZ:00253811</oboInOwl:id>
        <rdfs:label>Aroroa Island</rdfs:label>
    </owl:NamedIndividual>
    


    <!-- http://purl.obolibrary.org/obo/GAZ_00253812 -->

    <owl:NamedIndividual rdf:about="http://purl.obolibrary.org/obo/GAZ_00253812">
        <obo:RO_0001025 rdf:resource="http://purl.obolibrary.org/obo/GAZ_00253808"/>
        <obo:IAO_0000115>An island in the Conflict Group.</obo:IAO_0000115>
        <oboInOwl:hasOBONamespace>GAZ</oboInOwl:hasOBONamespace>
        <oboInOwl:id>GAZ:00253812</oboInOwl:id>
        <rdfs:label>Panarakuum Island</rdfs:label>
    </owl:NamedIndividual>
    


    <!-- http://purl.obolibrary.org/obo/GAZ_00253813 -->

    <owl:NamedIndividual rdf:about="http://purl.obolibrary.org/obo/GAZ_00253813">
        <obo:RO_0001025 rdf:resource="http://purl.obolibrary.org/obo/GAZ_00253808"/>
        <obo:IAO_0000115>An island in the Conflict Group.</obo:IAO_0000115>
        <oboInOwl:hasOBONamespace>GAZ</oboInOwl:hasOBONamespace>
        <oboInOwl:id>GAZ:00253813</oboInOwl:id>
        <rdfs:label>Panibari Island</rdfs:label>
    </owl:NamedIndividual>
    


    <!-- http://purl.obolibrary.org/obo/GAZ_00253814 -->

    <owl:NamedIndividual rdf:about="http://purl.obolibrary.org/obo/GAZ_00253814">
        <obo:RO_0001025 rdf:resource="http://purl.obolibrary.org/obo/GAZ_00253808"/>
        <obo:IAO_0000115>An island in the Conflict Group.</obo:IAO_0000115>
        <oboInOwl:hasOBONamespace>GAZ</oboInOwl:hasOBONamespace>
        <oboInOwl:id>GAZ:00253814</oboInOwl:id>
        <rdfs:label>Tubiniguam Island</rdfs:label>
    </owl:NamedIndividual>
    


    <!-- http://purl.obolibrary.org/obo/GAZ_00253815 -->

    <owl:NamedIndividual rdf:about="http://purl.obolibrary.org/obo/GAZ_00253815">
        <obo:RO_0001025 rdf:resource="http://purl.obolibrary.org/obo/GAZ_00253808"/>
        <obo:IAO_0000115>An island in the Conflict Group.</obo:IAO_0000115>
        <oboInOwl:hasOBONamespace>GAZ</oboInOwl:hasOBONamespace>
        <oboInOwl:id>GAZ:00253815</oboInOwl:id>
        <rdfs:label>Moniara Island</rdfs:label>
    </owl:NamedIndividual>
    


    <!-- http://purl.obolibrary.org/obo/GAZ_00253816 -->

    <owl:NamedIndividual rdf:about="http://purl.obolibrary.org/obo/GAZ_00253816">
        <obo:RO_0001025 rdf:resource="http://purl.obolibrary.org/obo/GAZ_00253808"/>
        <obo:IAO_0000115>An island in the Conflict Group.</obo:IAO_0000115>
        <oboInOwl:hasOBONamespace>GAZ</oboInOwl:hasOBONamespace>
        <oboInOwl:id>GAZ:00253816</oboInOwl:id>
        <rdfs:label>Ginouri Island</rdfs:label>
    </owl:NamedIndividual>
    


    <!-- http://purl.obolibrary.org/obo/GAZ_00253817 -->

    <owl:NamedIndividual rdf:about="http://purl.obolibrary.org/obo/GAZ_00253817">
        <obo:RO_0001025 rdf:resource="http://purl.obolibrary.org/obo/GAZ_00253808"/>
        <obo:IAO_0000115>An island in the Conflict Group.</obo:IAO_0000115>
        <oboInOwl:hasOBONamespace>GAZ</oboInOwl:hasOBONamespace>
        <oboInOwl:id>GAZ:00253817</oboInOwl:id>
        <rdfs:label>Tupit Island</rdfs:label>
    </owl:NamedIndividual>
    


    <!-- http://purl.obolibrary.org/obo/GAZ_00253818 -->

    <owl:NamedIndividual rdf:about="http://purl.obolibrary.org/obo/GAZ_00253818">
        <obo:RO_0001025 rdf:resource="http://purl.obolibrary.org/obo/GAZ_00007182"/>
        <obo:IAO_0000115>A group of large reefs and islands situated on the northern side of the Louisiade Archipelago, located 13 km southwest from Misima.</obo:IAO_0000115>
        <oboInOwl:hasOBONamespace>GAZ</oboInOwl:hasOBONamespace>
        <oboInOwl:id>GAZ:00253818</oboInOwl:id>
        <rdfs:label>Deboyne Islands</rdfs:label>
    </owl:NamedIndividual>
    


    <!-- http://purl.obolibrary.org/obo/GAZ_00253819 -->

    <owl:NamedIndividual rdf:about="http://purl.obolibrary.org/obo/GAZ_00253819">
        <obo:RO_0001025 rdf:resource="http://purl.obolibrary.org/obo/GAZ_00253818"/>
        <obo:IAO_0000115>One of the Deboyne Islands.</obo:IAO_0000115>
        <oboInOwl:hasOBONamespace>GAZ</oboInOwl:hasOBONamespace>
        <oboInOwl:id>GAZ:00253819</oboInOwl:id>
        <rdfs:label>Panaeati Island</rdfs:label>
    </owl:NamedIndividual>
    


    <!-- http://purl.obolibrary.org/obo/GAZ_00253820 -->

    <owl:NamedIndividual rdf:about="http://purl.obolibrary.org/obo/GAZ_00253820">
        <obo:RO_0001025 rdf:resource="http://purl.obolibrary.org/obo/GAZ_00253818"/>
        <obo:IAO_0000115>One of the Deboyne Islands.</obo:IAO_0000115>
        <oboInOwl:hasOBONamespace>GAZ</oboInOwl:hasOBONamespace>
        <oboInOwl:id>GAZ:00253820</oboInOwl:id>
        <rdfs:label>Panapompom Island</rdfs:label>
    </owl:NamedIndividual>
    


    <!-- http://purl.obolibrary.org/obo/GAZ_00253821 -->

    <owl:NamedIndividual rdf:about="http://purl.obolibrary.org/obo/GAZ_00253821">
        <obo:RO_0001025 rdf:resource="http://purl.obolibrary.org/obo/GAZ_00253818"/>
        <obo:IAO_0000115>One of the Deboyne Islands.</obo:IAO_0000115>
        <oboInOwl:hasOBONamespace>GAZ</oboInOwl:hasOBONamespace>
        <oboInOwl:id>GAZ:00253821</oboInOwl:id>
        <rdfs:label>Brooker Island</rdfs:label>
    </owl:NamedIndividual>
    


    <!-- http://purl.obolibrary.org/obo/GAZ_00253822 -->

    <owl:NamedIndividual rdf:about="http://purl.obolibrary.org/obo/GAZ_00253822">
        <obo:RO_0001025 rdf:resource="http://purl.obolibrary.org/obo/GAZ_00253818"/>
        <obo:IAO_0000115>One of the Deboyne Islands.</obo:IAO_0000115>
        <oboInOwl:hasOBONamespace>GAZ</oboInOwl:hasOBONamespace>
        <oboInOwl:id>GAZ:00253822</oboInOwl:id>
        <rdfs:label>Ware Island</rdfs:label>
    </owl:NamedIndividual>
    


    <!-- http://purl.obolibrary.org/obo/GAZ_00253823 -->

    <owl:NamedIndividual rdf:about="http://purl.obolibrary.org/obo/GAZ_00253823">
        <rdf:type rdf:resource="http://purl.obolibrary.org/obo/ENVO_00000220"/>
        <obo:RO_0001025 rdf:resource="http://purl.obolibrary.org/obo/GAZ_00007182"/>
        <obo:IAO_0000115>An island group that lies on the northern side of the Louisiade Archipelago, situated 21 km north from the outer barrier reefs of Vanatinai and 19 km southeast from Misima; the small Manuga Reef lies 19 km to the southeast.</obo:IAO_0000115>
        <oboInOwl:hasOBONamespace>GAZ</oboInOwl:hasOBONamespace>
        <oboInOwl:id>GAZ:00253823</oboInOwl:id>
        <rdfs:label>Renard Islands</rdfs:label>
    </owl:NamedIndividual>
    


    <!-- http://purl.obolibrary.org/obo/GAZ_00253824 -->

    <owl:NamedIndividual rdf:about="http://purl.obolibrary.org/obo/GAZ_00253824">
        <obo:RO_0001025 rdf:resource="http://purl.obolibrary.org/obo/GAZ_00253823"/>
        <obo:IAO_0000115>An island in the Renard Group.</obo:IAO_0000115>
        <oboInOwl:hasOBONamespace>GAZ</oboInOwl:hasOBONamespace>
        <oboInOwl:id>GAZ:00253824</oboInOwl:id>
        <rdfs:label>Kimuta Island</rdfs:label>
    </owl:NamedIndividual>
    


    <!-- http://purl.obolibrary.org/obo/GAZ_00253825 -->

    <owl:NamedIndividual rdf:about="http://purl.obolibrary.org/obo/GAZ_00253825">
        <obo:RO_0001025 rdf:resource="http://purl.obolibrary.org/obo/GAZ_00253823"/>
        <obo:IAO_0000115>An island in the Renard Group.</obo:IAO_0000115>
        <oboInOwl:hasOBONamespace>GAZ</oboInOwl:hasOBONamespace>
        <oboInOwl:id>GAZ:00253825</oboInOwl:id>
        <rdfs:label>Bagaium Island</rdfs:label>
    </owl:NamedIndividual>
    


    <!-- http://purl.obolibrary.org/obo/GAZ_00253826 -->

    <owl:NamedIndividual rdf:about="http://purl.obolibrary.org/obo/GAZ_00253826">
        <obo:RO_0001025 rdf:resource="http://purl.obolibrary.org/obo/GAZ_00253823"/>
        <obo:IAO_0000115>An island in the Renard Group.</obo:IAO_0000115>
        <oboInOwl:hasOBONamespace>GAZ</oboInOwl:hasOBONamespace>
        <oboInOwl:id>GAZ:00253826</oboInOwl:id>
        <rdfs:label>Niva BenoIsland</rdfs:label>
    </owl:NamedIndividual>
    


    <!-- http://purl.obolibrary.org/obo/GAZ_00253827 -->

    <owl:NamedIndividual rdf:about="http://purl.obolibrary.org/obo/GAZ_00253827">
        <obo:RO_0001025 rdf:resource="http://purl.obolibrary.org/obo/GAZ_00253823"/>
        <obo:IAO_0000115>An island in the Renard Group.</obo:IAO_0000115>
        <oboInOwl:hasOBONamespace>GAZ</oboInOwl:hasOBONamespace>
        <oboInOwl:id>GAZ:00253827</oboInOwl:id>
        <rdfs:label>Topuna Island</rdfs:label>
    </owl:NamedIndividual>
    


    <!-- http://purl.obolibrary.org/obo/GAZ_00253828 -->

    <owl:NamedIndividual rdf:about="http://purl.obolibrary.org/obo/GAZ_00253828">
        <obo:RO_0001025 rdf:resource="http://purl.obolibrary.org/obo/GAZ_00253823"/>
        <obo:IAO_0000115>An island in the Renard Group.</obo:IAO_0000115>
        <oboInOwl:hasOBONamespace>GAZ</oboInOwl:hasOBONamespace>
        <oboInOwl:id>GAZ:00253828</oboInOwl:id>
        <rdfs:label>Baiwa Island</rdfs:label>
    </owl:NamedIndividual>
    


    <!-- http://purl.obolibrary.org/obo/GAZ_00253829 -->

    <owl:NamedIndividual rdf:about="http://purl.obolibrary.org/obo/GAZ_00253829">
        <obo:RO_0001025 rdf:resource="http://purl.obolibrary.org/obo/GAZ_00253823"/>
        <obo:IAO_0000115>An island in the Renard Group.</obo:IAO_0000115>
        <oboInOwl:hasOBONamespace>GAZ</oboInOwl:hasOBONamespace>
        <oboInOwl:id>GAZ:00253829</oboInOwl:id>
        <rdfs:label>Oreia Islet</rdfs:label>
    </owl:NamedIndividual>
    


    <!-- http://purl.obolibrary.org/obo/GAZ_00253830 -->

    <owl:NamedIndividual rdf:about="http://purl.obolibrary.org/obo/GAZ_00253830">
        <obo:RO_0001025 rdf:resource="http://purl.obolibrary.org/obo/GAZ_00253823"/>
        <obo:IAO_0000115>An island in the Renard Group.</obo:IAO_0000115>
        <oboInOwl:hasOBONamespace>GAZ</oboInOwl:hasOBONamespace>
        <oboInOwl:id>GAZ:00253830</oboInOwl:id>
        <rdfs:label>Epoko Islet</rdfs:label>
    </owl:NamedIndividual>
    


    <!-- http://purl.obolibrary.org/obo/GAZ_00253831 -->

    <owl:NamedIndividual rdf:about="http://purl.obolibrary.org/obo/GAZ_00253831">
        <obo:RO_0001025 rdf:resource="http://purl.obolibrary.org/obo/GAZ_00253823"/>
        <obo:IAO_0000115>An island in the Renard Group.</obo:IAO_0000115>
        <oboInOwl:hasOBONamespace>GAZ</oboInOwl:hasOBONamespace>
        <oboInOwl:id>GAZ:00253831</oboInOwl:id>
        <rdfs:label>Pana Wadai</rdfs:label>
    </owl:NamedIndividual>
    


    <!-- http://purl.obolibrary.org/obo/GAZ_00253832 -->

    <owl:NamedIndividual rdf:about="http://purl.obolibrary.org/obo/GAZ_00253832">
        <obo:RO_0001025 rdf:resource="http://purl.obolibrary.org/obo/GAZ_00253823"/>
        <obo:IAO_0000115>An island in the Renard Group.</obo:IAO_0000115>
        <oboInOwl:hasOBONamespace>GAZ</oboInOwl:hasOBONamespace>
        <oboInOwl:id>GAZ:00253832</oboInOwl:id>
        <rdfs:label>Pana Roran</rdfs:label>
    </owl:NamedIndividual>
    


    <!-- http://purl.obolibrary.org/obo/GAZ_00253833 -->

    <owl:NamedIndividual rdf:about="http://purl.obolibrary.org/obo/GAZ_00253833">
        <obo:RO_0001025 rdf:resource="http://purl.obolibrary.org/obo/GAZ_00007182"/>
        <obo:IAO_0000115>A minor reef system of the Louisiade Archipelago, the linear Manuga Reef is located 20 km northeast from the Vanatinai barrier reef and 19 km southeast from the Renard Islands. The reef has two components: a larger reef on the southeast (6 km in length) and a smaller reef on the northwest (3 km in length). The northeastern reef contains three small sand cays.</obo:IAO_0000115>
        <oboInOwl:hasOBONamespace>GAZ</oboInOwl:hasOBONamespace>
        <oboInOwl:id>GAZ:00253833</oboInOwl:id>
        <rdfs:label>Manuga Reef</rdfs:label>
    </owl:NamedIndividual>
    


    <!-- http://purl.obolibrary.org/obo/GAZ_00253834 -->

    <owl:NamedIndividual rdf:about="http://purl.obolibrary.org/obo/GAZ_00253834">
        <obo:RO_0001025 rdf:resource="http://purl.obolibrary.org/obo/GAZ_00007182"/>
        <obo:IAO_0000115>An atoll-like reef of the Louisiade Archipelago, Long Reef is the largest component of a chain of major reef formations, Bramble Haven, Long Reef and the Anchorage Reefs, that extend westwards from the western edge of the Vanatinai barrier reef.</obo:IAO_0000115>
        <oboInOwl:hasOBONamespace>GAZ</oboInOwl:hasOBONamespace>
        <oboInOwl:id>GAZ:00253834</oboInOwl:id>
        <rdfs:label>Long Reef</rdfs:label>
    </owl:NamedIndividual>
    


    <!-- http://purl.obolibrary.org/obo/GAZ_00253835 -->

    <owl:NamedIndividual rdf:about="http://purl.obolibrary.org/obo/GAZ_00253835">
        <obo:RO_0001025 rdf:resource="http://purl.obolibrary.org/obo/GAZ_00007182"/>
        <obo:IAO_0000115>A reef system of the Louisiade Archipelago, Bramble Haven is the easternmost section of an extensive chain of atolls, reefs and islands that extend from the western side of Vanatinai&apos;s southern barrier reef; the reefs ultimately continue to the west for over 400 km, wrapping around the southern coast of the Papuan Peninsula.</obo:IAO_0000115>
        <oboInOwl:hasOBONamespace>GAZ</oboInOwl:hasOBONamespace>
        <oboInOwl:id>GAZ:00253835</oboInOwl:id>
        <rdfs:label>Bramble Haven</rdfs:label>
    </owl:NamedIndividual>
    


    <!-- http://purl.obolibrary.org/obo/GAZ_00253836 -->

    <owl:NamedIndividual rdf:about="http://purl.obolibrary.org/obo/GAZ_00253836">
        <obo:RO_0001025 rdf:resource="http://purl.obolibrary.org/obo/GAZ_00253835"/>
        <obo:IAO_0000115>A group of small islands on the N edge of Bramble Haven.</obo:IAO_0000115>
        <oboInOwl:hasOBONamespace>GAZ</oboInOwl:hasOBONamespace>
        <oboInOwl:id>GAZ:00253836</oboInOwl:id>
        <rdfs:label>Duperre Islets</rdfs:label>
    </owl:NamedIndividual>
    


    <!-- http://purl.obolibrary.org/obo/GAZ_00253837 -->

    <owl:NamedIndividual rdf:about="http://purl.obolibrary.org/obo/GAZ_00253837">
        <obo:RO_0001025 rdf:resource="http://purl.obolibrary.org/obo/GAZ_00253836"/>
        <obo:IAO_0000115>One of the Duperre Islets.</obo:IAO_0000115>
        <oboInOwl:hasOBONamespace>GAZ</oboInOwl:hasOBONamespace>
        <oboInOwl:id>GAZ:00253837</oboInOwl:id>
        <rdfs:label>Punawan</rdfs:label>
    </owl:NamedIndividual>
    


    <!-- http://purl.obolibrary.org/obo/GAZ_00253838 -->

    <owl:NamedIndividual rdf:about="http://purl.obolibrary.org/obo/GAZ_00253838">
        <obo:RO_0001025 rdf:resource="http://purl.obolibrary.org/obo/GAZ_00253836"/>
        <obo:IAO_0000115>One of the Duperre Islets.</obo:IAO_0000115>
        <oboInOwl:hasOBONamespace>GAZ</oboInOwl:hasOBONamespace>
        <oboInOwl:id>GAZ:00253838</oboInOwl:id>
        <rdfs:label>Duperre Islet</rdfs:label>
    </owl:NamedIndividual>
    


    <!-- http://purl.obolibrary.org/obo/GAZ_00253839 -->

    <owl:NamedIndividual rdf:about="http://purl.obolibrary.org/obo/GAZ_00253839">
        <obo:RO_0001025 rdf:resource="http://purl.obolibrary.org/obo/GAZ_00253836"/>
        <obo:IAO_0000115>One of the Duperre Islets.</obo:IAO_0000115>
        <oboInOwl:hasOBONamespace>GAZ</oboInOwl:hasOBONamespace>
        <oboInOwl:id>GAZ:00253839</oboInOwl:id>
        <rdfs:label>Siva</rdfs:label>
    </owl:NamedIndividual>
    


    <!-- http://purl.obolibrary.org/obo/GAZ_00253840 -->

    <owl:NamedIndividual rdf:about="http://purl.obolibrary.org/obo/GAZ_00253840">
        <obo:RO_0001025 rdf:resource="http://purl.obolibrary.org/obo/GAZ_00253836"/>
        <obo:IAO_0000115>One of the Duperre Islets.</obo:IAO_0000115>
        <oboInOwl:hasOBONamespace>GAZ</oboInOwl:hasOBONamespace>
        <oboInOwl:id>GAZ:00253840</oboInOwl:id>
        <rdfs:label>Panapwa</rdfs:label>
    </owl:NamedIndividual>
    


    <!-- http://purl.obolibrary.org/obo/GAZ_00253841 -->

    <owl:NamedIndividual rdf:about="http://purl.obolibrary.org/obo/GAZ_00253841">
        <obo:RO_0001025 rdf:resource="http://purl.obolibrary.org/obo/GAZ_00253836"/>
        <obo:IAO_0000115>One of the Duperre Islets.</obo:IAO_0000115>
        <oboInOwl:hasOBONamespace>GAZ</oboInOwl:hasOBONamespace>
        <oboInOwl:id>GAZ:00253841</oboInOwl:id>
        <rdfs:label>Awanagamwana</rdfs:label>
    </owl:NamedIndividual>
    


    <!-- http://purl.obolibrary.org/obo/GAZ_00253842 -->

    <owl:NamedIndividual rdf:about="http://purl.obolibrary.org/obo/GAZ_00253842">
        <obo:RO_0001025 rdf:resource="http://purl.obolibrary.org/obo/GAZ_00007182"/>
        <obo:IAO_0000115>Two islands located at the southern side of the deep Jomard Entrance, the 9 km wide passage between Bramble Haven and the western edge of the Vanatinai barrier reef. The islands thus form part of the Louisiade Archipelago.</obo:IAO_0000115>
        <oboInOwl:hasOBONamespace>GAZ</oboInOwl:hasOBONamespace>
        <oboInOwl:id>GAZ:00253842</oboInOwl:id>
        <rdfs:label>Jomard Islands</rdfs:label>
    </owl:NamedIndividual>
    


    <!-- http://purl.obolibrary.org/obo/GAZ_00253843 -->

    <owl:NamedIndividual rdf:about="http://purl.obolibrary.org/obo/GAZ_00253843">
        <obo:RO_0001025 rdf:resource="http://purl.obolibrary.org/obo/GAZ_00253842"/>
        <obo:IAO_0000115>The larger of the two Jomard Islands.</obo:IAO_0000115>
        <oboInOwl:hasOBONamespace>GAZ</oboInOwl:hasOBONamespace>
        <oboInOwl:id>GAZ:00253843</oboInOwl:id>
        <rdfs:label>Pana Waipona</rdfs:label>
    </owl:NamedIndividual>
    


    <!-- http://purl.obolibrary.org/obo/GAZ_00253844 -->

    <owl:NamedIndividual rdf:about="http://purl.obolibrary.org/obo/GAZ_00253844">
        <obo:RO_0001025 rdf:resource="http://purl.obolibrary.org/obo/GAZ_00253842"/>
        <obo:IAO_0000115>The smaller of the two Jomard Islands.</obo:IAO_0000115>
        <oboInOwl:hasOBONamespace>GAZ</oboInOwl:hasOBONamespace>
        <oboInOwl:id>GAZ:00253844</oboInOwl:id>
        <rdfs:label>Pana Rai Rai</rdfs:label>
    </owl:NamedIndividual>
    


    <!-- http://purl.obolibrary.org/obo/GAZ_00253845 -->

    <owl:NamedIndividual rdf:about="http://purl.obolibrary.org/obo/GAZ_00253845">
        <obo:RO_0001025 rdf:resource="http://purl.obolibrary.org/obo/GAZ_00007182"/>
        <obo:IAO_0000115>Islands that are located within the lagoon of the Vanatinai island-barrier reef system. The islands extend in an easterly direction from Panasia (off Pana Tinani) to Hemenahei, across a distance of some 80 km.</obo:IAO_0000115>
        <oboInOwl:hasOBONamespace>GAZ</oboInOwl:hasOBONamespace>
        <oboInOwl:id>GAZ:00253845</oboInOwl:id>
        <rdfs:label>Calvados Chain</rdfs:label>
    </owl:NamedIndividual>
    


    <!-- http://purl.obolibrary.org/obo/GAZ_00253846 -->

    <owl:NamedIndividual rdf:about="http://purl.obolibrary.org/obo/GAZ_00253846">
        <obo:RO_0001025 rdf:resource="http://purl.obolibrary.org/obo/GAZ_00253845"/>
        <obo:IAO_0000115>An island of the Cavalier Chain.</obo:IAO_0000115>
        <oboInOwl:hasOBONamespace>GAZ</oboInOwl:hasOBONamespace>
        <oboInOwl:id>GAZ:00253846</oboInOwl:id>
        <rdfs:label>Pana Vara Vara</rdfs:label>
    </owl:NamedIndividual>
    


    <!-- http://purl.obolibrary.org/obo/GAZ_00253847 -->

    <owl:NamedIndividual rdf:about="http://purl.obolibrary.org/obo/GAZ_00253847">
        <obo:RO_0001025 rdf:resource="http://purl.obolibrary.org/obo/GAZ_00253845"/>
        <obo:IAO_0000115>An island of the Cavalier Chain.</obo:IAO_0000115>
        <oboInOwl:hasOBONamespace>GAZ</oboInOwl:hasOBONamespace>
        <oboInOwl:id>GAZ:00253847</oboInOwl:id>
        <rdfs:label>Pana Rai Rai</rdfs:label>
    </owl:NamedIndividual>
    


    <!-- http://purl.obolibrary.org/obo/GAZ_00253848 -->

    <owl:NamedIndividual rdf:about="http://purl.obolibrary.org/obo/GAZ_00253848">
        <obo:RO_0001025 rdf:resource="http://purl.obolibrary.org/obo/GAZ_00253845"/>
        <obo:IAO_0000115>An island of the Cavalier Chain.</obo:IAO_0000115>
        <oboInOwl:hasOBONamespace>GAZ</oboInOwl:hasOBONamespace>
        <oboInOwl:id>GAZ:00253848</oboInOwl:id>
        <rdfs:label>Utian Panarora</rdfs:label>
    </owl:NamedIndividual>
    


    <!-- http://purl.obolibrary.org/obo/GAZ_00253849 -->

    <owl:NamedIndividual rdf:about="http://purl.obolibrary.org/obo/GAZ_00253849">
        <obo:RO_0001025 rdf:resource="http://purl.obolibrary.org/obo/GAZ_00253845"/>
        <obo:IAO_0000115>An island of the Cavalier Chain.</obo:IAO_0000115>
        <oboInOwl:hasOBONamespace>GAZ</oboInOwl:hasOBONamespace>
        <oboInOwl:id>GAZ:00253849</oboInOwl:id>
        <rdfs:label>Pana Udu Udi</rdfs:label>
    </owl:NamedIndividual>
    


    <!-- http://purl.obolibrary.org/obo/GAZ_00253850 -->

    <owl:NamedIndividual rdf:about="http://purl.obolibrary.org/obo/GAZ_00253850">
        <obo:RO_0001025 rdf:resource="http://purl.obolibrary.org/obo/GAZ_00253845"/>
        <obo:IAO_0000115>An island of the Cavalier Chain.</obo:IAO_0000115>
        <oboInOwl:hasOBONamespace>GAZ</oboInOwl:hasOBONamespace>
        <oboInOwl:id>GAZ:00253850</oboInOwl:id>
        <rdfs:label>Gulewa Island</rdfs:label>
    </owl:NamedIndividual>
    


    <!-- http://purl.obolibrary.org/obo/GAZ_00253851 -->

    <owl:NamedIndividual rdf:about="http://purl.obolibrary.org/obo/GAZ_00253851">
        <obo:RO_0001025 rdf:resource="http://purl.obolibrary.org/obo/GAZ_00253845"/>
        <obo:IAO_0000115>An island of the Cavalier Chain.</obo:IAO_0000115>
        <oboInOwl:hasOBONamespace>GAZ</oboInOwl:hasOBONamespace>
        <oboInOwl:id>GAZ:00253851</oboInOwl:id>
        <rdfs:label>Moturina Island</rdfs:label>
    </owl:NamedIndividual>
    


    <!-- http://purl.obolibrary.org/obo/GAZ_00253852 -->

    <owl:NamedIndividual rdf:about="http://purl.obolibrary.org/obo/GAZ_00253852">
        <obo:RO_0001025 rdf:resource="http://purl.obolibrary.org/obo/GAZ_00253845"/>
        <obo:IAO_0000115>An island of the Cavalier Chain.</obo:IAO_0000115>
        <oboInOwl:hasOBONamespace>GAZ</oboInOwl:hasOBONamespace>
        <oboInOwl:id>GAZ:00253852</oboInOwl:id>
        <rdfs:label>Ululina Island</rdfs:label>
    </owl:NamedIndividual>
    


    <!-- http://purl.obolibrary.org/obo/GAZ_00253853 -->

    <owl:NamedIndividual rdf:about="http://purl.obolibrary.org/obo/GAZ_00253853">
        <obo:RO_0001025 rdf:resource="http://purl.obolibrary.org/obo/GAZ_00253845"/>
        <obo:IAO_0000115>An island of the Cavalier Chain.</obo:IAO_0000115>
        <oboInOwl:hasOBONamespace>GAZ</oboInOwl:hasOBONamespace>
        <oboInOwl:id>GAZ:00253853</oboInOwl:id>
        <rdfs:label>Venariwa Island</rdfs:label>
    </owl:NamedIndividual>
    


    <!-- http://purl.obolibrary.org/obo/GAZ_00253854 -->

    <owl:NamedIndividual rdf:about="http://purl.obolibrary.org/obo/GAZ_00253854">
        <obo:RO_0001025 rdf:resource="http://purl.obolibrary.org/obo/GAZ_00253845"/>
        <obo:IAO_0000115>An island of the Cavalier Chain.</obo:IAO_0000115>
        <oboInOwl:hasOBONamespace>GAZ</oboInOwl:hasOBONamespace>
        <oboInOwl:id>GAZ:00253854</oboInOwl:id>
        <rdfs:label>Bonna Wan Island</rdfs:label>
    </owl:NamedIndividual>
    


    <!-- http://purl.obolibrary.org/obo/GAZ_00253855 -->

    <owl:NamedIndividual rdf:about="http://purl.obolibrary.org/obo/GAZ_00253855">
        <obo:RO_0001025 rdf:resource="http://purl.obolibrary.org/obo/GAZ_00253845"/>
        <obo:IAO_0000115>An island of the Cavalier Chain.</obo:IAO_0000115>
        <oboInOwl:hasOBONamespace>GAZ</oboInOwl:hasOBONamespace>
        <oboInOwl:id>GAZ:00253855</oboInOwl:id>
        <rdfs:label>Bagaman Island</rdfs:label>
    </owl:NamedIndividual>
    


    <!-- http://purl.obolibrary.org/obo/GAZ_00253856 -->

    <owl:NamedIndividual rdf:about="http://purl.obolibrary.org/obo/GAZ_00253856">
        <obo:RO_0001025 rdf:resource="http://purl.obolibrary.org/obo/GAZ_00253845"/>
        <obo:IAO_0000115>An island of the Cavalier Chain.</obo:IAO_0000115>
        <oboInOwl:hasOBONamespace>GAZ</oboInOwl:hasOBONamespace>
        <oboInOwl:id>GAZ:00253856</oboInOwl:id>
        <rdfs:label>Bobo Eina Island</rdfs:label>
    </owl:NamedIndividual>
    


    <!-- http://purl.obolibrary.org/obo/GAZ_00253857 -->

    <owl:NamedIndividual rdf:about="http://purl.obolibrary.org/obo/GAZ_00253857">
        <obo:RO_0001025 rdf:resource="http://purl.obolibrary.org/obo/GAZ_00253845"/>
        <obo:IAO_0000115>An island of the Cavalier Chain.</obo:IAO_0000115>
        <oboInOwl:hasOBONamespace>GAZ</oboInOwl:hasOBONamespace>
        <oboInOwl:id>GAZ:00253857</oboInOwl:id>
        <rdfs:label>Pana Numara</rdfs:label>
    </owl:NamedIndividual>
    


    <!-- http://purl.obolibrary.org/obo/GAZ_00253858 -->

    <owl:NamedIndividual rdf:about="http://purl.obolibrary.org/obo/GAZ_00253858">
        <obo:RO_0001025 rdf:resource="http://purl.obolibrary.org/obo/GAZ_00253845"/>
        <obo:IAO_0000115>An island of the Cavalier Chain.</obo:IAO_0000115>
        <oboInOwl:hasOBONamespace>GAZ</oboInOwl:hasOBONamespace>
        <oboInOwl:id>GAZ:00253858</oboInOwl:id>
        <rdfs:label>Yaruman Island</rdfs:label>
    </owl:NamedIndividual>
    


    <!-- http://purl.obolibrary.org/obo/GAZ_00253859 -->

    <owl:NamedIndividual rdf:about="http://purl.obolibrary.org/obo/GAZ_00253859">
        <obo:RO_0001025 rdf:resource="http://purl.obolibrary.org/obo/GAZ_00253845"/>
        <obo:IAO_0000115>An island of the Cavalier Chain.</obo:IAO_0000115>
        <oboInOwl:hasOBONamespace>GAZ</oboInOwl:hasOBONamespace>
        <oboInOwl:id>GAZ:00253859</oboInOwl:id>
        <rdfs:label>Panangaribu</rdfs:label>
    </owl:NamedIndividual>
    


    <!-- http://purl.obolibrary.org/obo/GAZ_00253860 -->

    <owl:NamedIndividual rdf:about="http://purl.obolibrary.org/obo/GAZ_00253860">
        <obo:RO_0001025 rdf:resource="http://purl.obolibrary.org/obo/GAZ_00253845"/>
        <obo:IAO_0000115>An island of the Cavalier Chain.</obo:IAO_0000115>
        <oboInOwl:hasOBONamespace>GAZ</oboInOwl:hasOBONamespace>
        <oboInOwl:id>GAZ:00253860</oboInOwl:id>
        <rdfs:label>Panantanian</rdfs:label>
    </owl:NamedIndividual>
    


    <!-- http://purl.obolibrary.org/obo/GAZ_00253861 -->

    <owl:NamedIndividual rdf:about="http://purl.obolibrary.org/obo/GAZ_00253861">
        <obo:RO_0001025 rdf:resource="http://purl.obolibrary.org/obo/GAZ_00253845"/>
        <obo:IAO_0000115>An island of the Cavalier Chain.</obo:IAO_0000115>
        <oboInOwl:hasOBONamespace>GAZ</oboInOwl:hasOBONamespace>
        <oboInOwl:id>GAZ:00253861</oboInOwl:id>
        <rdfs:label>Pana Krusima</rdfs:label>
    </owl:NamedIndividual>
    


    <!-- http://purl.obolibrary.org/obo/GAZ_00253862 -->

    <owl:NamedIndividual rdf:about="http://purl.obolibrary.org/obo/GAZ_00253862">
        <obo:RO_0001025 rdf:resource="http://purl.obolibrary.org/obo/GAZ_00253845"/>
        <obo:IAO_0000115>An island of the Cavalier Chain.</obo:IAO_0000115>
        <oboInOwl:hasOBONamespace>GAZ</oboInOwl:hasOBONamespace>
        <oboInOwl:id>GAZ:00253862</oboInOwl:id>
        <rdfs:label>Kuanak Island</rdfs:label>
    </owl:NamedIndividual>
    


    <!-- http://purl.obolibrary.org/obo/GAZ_00253863 -->

    <owl:NamedIndividual rdf:about="http://purl.obolibrary.org/obo/GAZ_00253863">
        <obo:RO_0001025 rdf:resource="http://purl.obolibrary.org/obo/GAZ_00253845"/>
        <obo:IAO_0000115>An island of the Cavalier Chain.</obo:IAO_0000115>
        <oboInOwl:hasOBONamespace>GAZ</oboInOwl:hasOBONamespace>
        <oboInOwl:id>GAZ:00253863</oboInOwl:id>
        <rdfs:label>Gigila Island</rdfs:label>
    </owl:NamedIndividual>
    


    <!-- http://purl.obolibrary.org/obo/GAZ_00253864 -->

    <owl:NamedIndividual rdf:about="http://purl.obolibrary.org/obo/GAZ_00253864">
        <obo:RO_0001025 rdf:resource="http://purl.obolibrary.org/obo/GAZ_00253845"/>
        <obo:IAO_0000115>An island of the Cavalier Chain.</obo:IAO_0000115>
        <oboInOwl:hasOBONamespace>GAZ</oboInOwl:hasOBONamespace>
        <oboInOwl:id>GAZ:00253864</oboInOwl:id>
        <rdfs:label>Pana Wina</rdfs:label>
    </owl:NamedIndividual>
    


    <!-- http://purl.obolibrary.org/obo/GAZ_00253865 -->

    <owl:NamedIndividual rdf:about="http://purl.obolibrary.org/obo/GAZ_00253865">
        <rdf:type rdf:resource="http://purl.obolibrary.org/obo/ENVO_00000130"/>
        <obo:RO_0001025 rdf:resource="http://purl.obolibrary.org/obo/GAZ_00253845"/>
        <obo:IAO_0000115>A barrier reef.</obo:IAO_0000115>
        <oboInOwl:hasOBONamespace>GAZ</oboInOwl:hasOBONamespace>
        <oboInOwl:id>GAZ:00253865</oboInOwl:id>
        <rdfs:label>Calvados Barrier Reef</rdfs:label>
    </owl:NamedIndividual>
    


    <!-- http://purl.obolibrary.org/obo/GAZ_00253866 -->

    <owl:NamedIndividual rdf:about="http://purl.obolibrary.org/obo/GAZ_00253866">
        <obo:RO_0001025 rdf:resource="http://purl.obolibrary.org/obo/GAZ_00012666"/>
        <obo:IAO_0000115>A large, approximately circular-shaped, reef formation measuring 33 km by 20 km. It is located 50 km southwest from the Woodlark Islands and 82 km northeast from Normanby Island (in the D&apos;entrecasteaux Islands). Not an atoll but a reef-topped carbonate bank.</obo:IAO_0000115>
        <oboInOwl:hasOBONamespace>GAZ</oboInOwl:hasOBONamespace>
        <oboInOwl:id>GAZ:00253866</oboInOwl:id>
        <rdfs:label>Egum Atoll</rdfs:label>
    </owl:NamedIndividual>
    


    <!-- http://purl.obolibrary.org/obo/GAZ_00253867 -->

    <owl:NamedIndividual rdf:about="http://purl.obolibrary.org/obo/GAZ_00253867">
        <obo:RO_0001025 rdf:resource="http://purl.obolibrary.org/obo/GAZ_00012666"/>
        <obo:IAO_0000115>An atoll. Located SE of Woodlark Island.</obo:IAO_0000115>
        <oboInOwl:hasOBONamespace>GAZ</oboInOwl:hasOBONamespace>
        <oboInOwl:id>GAZ:00253867</oboInOwl:id>
        <rdfs:label>Budi Budi Atoll</rdfs:label>
    </owl:NamedIndividual>
    


    <!-- http://purl.obolibrary.org/obo/GAZ_00253868 -->

    <owl:NamedIndividual rdf:about="http://purl.obolibrary.org/obo/GAZ_00253868">
        <obo:RO_0001025 rdf:resource="http://purl.obolibrary.org/obo/GAZ_00007182"/>
        <obo:IAO_0000115>A small group of three low-lying islands located on the southwestern corner of the Vanatinai barrier reef; they are located 5 km southeast from the Jomard Islands and immediately northeast from the Montemont Islands.</obo:IAO_0000115>
        <oboInOwl:hasOBONamespace>GAZ</oboInOwl:hasOBONamespace>
        <oboInOwl:id>GAZ:00253868</oboInOwl:id>
        <rdfs:label>Duchateau Islands</rdfs:label>
    </owl:NamedIndividual>
    


    <!-- http://purl.obolibrary.org/obo/GAZ_00253869 -->

    <owl:NamedIndividual rdf:about="http://purl.obolibrary.org/obo/GAZ_00253869">
        <obo:RO_0001025 rdf:resource="http://purl.obolibrary.org/obo/GAZ_00253868"/>
        <obo:IAO_0000115>An island of the Duchateau Group.</obo:IAO_0000115>
        <oboInOwl:hasOBONamespace>GAZ</oboInOwl:hasOBONamespace>
        <oboInOwl:id>GAZ:00253869</oboInOwl:id>
        <rdfs:label>Pana Bobai Ana</rdfs:label>
    </owl:NamedIndividual>
    


    <!-- http://purl.obolibrary.org/obo/GAZ_00253870 -->

    <owl:NamedIndividual rdf:about="http://purl.obolibrary.org/obo/GAZ_00253870">
        <obo:RO_0001025 rdf:resource="http://purl.obolibrary.org/obo/GAZ_00253868"/>
        <obo:IAO_0000115>An island of the Duchateau Group.</obo:IAO_0000115>
        <oboInOwl:hasOBONamespace>GAZ</oboInOwl:hasOBONamespace>
        <oboInOwl:id>GAZ:00253870</oboInOwl:id>
        <rdfs:label>Pana Rura Wara</rdfs:label>
    </owl:NamedIndividual>
    


    <!-- http://purl.obolibrary.org/obo/GAZ_00253871 -->

    <owl:NamedIndividual rdf:about="http://purl.obolibrary.org/obo/GAZ_00253871">
        <obo:RO_0001025 rdf:resource="http://purl.obolibrary.org/obo/GAZ_00253868"/>
        <obo:IAO_0000115>An island of the Duchateau Group.</obo:IAO_0000115>
        <oboInOwl:hasOBONamespace>GAZ</oboInOwl:hasOBONamespace>
        <oboInOwl:id>GAZ:00253871</oboInOwl:id>
        <rdfs:label>Kukuluba Island</rdfs:label>
    </owl:NamedIndividual>
    


    <!-- http://purl.obolibrary.org/obo/GAZ_00253872 -->

    <owl:NamedIndividual rdf:about="http://purl.obolibrary.org/obo/GAZ_00253872">
        <obo:RO_0001025 rdf:resource="http://purl.obolibrary.org/obo/GAZ_00007182"/>
        <obo:IAO_0000115>Island located in the western reaches of the Louisiade Archipelago; situated 27 km south from Sideia.</obo:IAO_0000115>
        <oboInOwl:hasOBONamespace>GAZ</oboInOwl:hasOBONamespace>
        <oboInOwl:id>GAZ:00253872</oboInOwl:id>
        <rdfs:label>Dumoulin Islands</rdfs:label>
    </owl:NamedIndividual>
    


    <!-- http://purl.obolibrary.org/obo/GAZ_00253873 -->

    <owl:NamedIndividual rdf:about="http://purl.obolibrary.org/obo/GAZ_00253873">
        <obo:RO_0001025 rdf:resource="http://purl.obolibrary.org/obo/GAZ_00253872"/>
        <obo:IAO_0000115>An island.</obo:IAO_0000115>
        <oboInOwl:hasOBONamespace>GAZ</oboInOwl:hasOBONamespace>
        <oboInOwl:id>GAZ:00253873</oboInOwl:id>
        <rdfs:label>Baiiri Island</rdfs:label>
    </owl:NamedIndividual>
    


    <!-- http://purl.obolibrary.org/obo/GAZ_00253874 -->

    <owl:NamedIndividual rdf:about="http://purl.obolibrary.org/obo/GAZ_00253874">
        <obo:RO_0001025 rdf:resource="http://purl.obolibrary.org/obo/GAZ_00253872"/>
        <obo:IAO_0000115>An island.</obo:IAO_0000115>
        <oboInOwl:hasOBONamespace>GAZ</oboInOwl:hasOBONamespace>
        <oboInOwl:id>GAZ:00253874</oboInOwl:id>
        <rdfs:label>Ana Karu Karua</rdfs:label>
    </owl:NamedIndividual>
    


    <!-- http://purl.obolibrary.org/obo/GAZ_00253875 -->

    <owl:NamedIndividual rdf:about="http://purl.obolibrary.org/obo/GAZ_00253875">
        <obo:RO_0001025 rdf:resource="http://purl.obolibrary.org/obo/GAZ_00007182"/>
        <obo:IAO_0000115>Shoals located to the south of Sideia and north from the tiny islands of the Dumoulin Islands group.</obo:IAO_0000115>
        <oboInOwl:hasOBONamespace>GAZ</oboInOwl:hasOBONamespace>
        <oboInOwl:id>GAZ:00253875</oboInOwl:id>
        <rdfs:label>Siriki Shoals</rdfs:label>
    </owl:NamedIndividual>
    


    <!-- http://purl.obolibrary.org/obo/GAZ_00253876 -->

    <owl:NamedIndividual rdf:about="http://purl.obolibrary.org/obo/GAZ_00253876">
        <obo:RO_0001025 rdf:resource="http://purl.obolibrary.org/obo/GAZ_00051597"/>
        <obo:IAO_0000115>One of the Engineer Islands.</obo:IAO_0000115>
        <oboInOwl:hasOBONamespace>GAZ</oboInOwl:hasOBONamespace>
        <oboInOwl:id>GAZ:00253876</oboInOwl:id>
        <rdfs:label>Slade Island</rdfs:label>
    </owl:NamedIndividual>
    


    <!-- http://purl.obolibrary.org/obo/GAZ_00253877 -->

    <owl:NamedIndividual rdf:about="http://purl.obolibrary.org/obo/GAZ_00253877">
        <obo:RO_0001025 rdf:resource="http://purl.obolibrary.org/obo/GAZ_00051597"/>
        <obo:IAO_0000115>One of the Engineer Islands.</obo:IAO_0000115>
        <oboInOwl:hasOBONamespace>GAZ</oboInOwl:hasOBONamespace>
        <oboInOwl:id>GAZ:00253877</oboInOwl:id>
        <rdfs:label>Skelton Island</rdfs:label>
    </owl:NamedIndividual>
    


    <!-- http://purl.obolibrary.org/obo/GAZ_00253878 -->

    <owl:NamedIndividual rdf:about="http://purl.obolibrary.org/obo/GAZ_00253878">
        <obo:RO_0001025 rdf:resource="http://purl.obolibrary.org/obo/GAZ_00051597"/>
        <obo:IAO_0000115>One of the Engineer Islands.</obo:IAO_0000115>
        <oboInOwl:hasOBONamespace>GAZ</oboInOwl:hasOBONamespace>
        <oboInOwl:id>GAZ:00253878</oboInOwl:id>
        <rdfs:label>Watts Island</rdfs:label>
    </owl:NamedIndividual>
    


    <!-- http://purl.obolibrary.org/obo/GAZ_00253879 -->

    <owl:NamedIndividual rdf:about="http://purl.obolibrary.org/obo/GAZ_00253879">
        <obo:RO_0001025 rdf:resource="http://purl.obolibrary.org/obo/GAZ_00051597"/>
        <obo:IAO_0000115>One of the Engineer Islands.</obo:IAO_0000115>
        <oboInOwl:hasOBONamespace>GAZ</oboInOwl:hasOBONamespace>
        <oboInOwl:id>GAZ:00253879</oboInOwl:id>
        <rdfs:label>Hummock Island</rdfs:label>
    </owl:NamedIndividual>
    


    <!-- http://purl.obolibrary.org/obo/GAZ_00253880 -->

    <owl:NamedIndividual rdf:about="http://purl.obolibrary.org/obo/GAZ_00253880">
        <obo:RO_0001025 rdf:resource="http://purl.obolibrary.org/obo/GAZ_00051597"/>
        <obo:IAO_0000115>One of the Engineer Islands.</obo:IAO_0000115>
        <oboInOwl:hasOBONamespace>GAZ</oboInOwl:hasOBONamespace>
        <oboInOwl:id>GAZ:00253880</oboInOwl:id>
        <rdfs:label>Haszar Island</rdfs:label>
    </owl:NamedIndividual>
    


    <!-- http://purl.obolibrary.org/obo/GAZ_00253881 -->

    <owl:NamedIndividual rdf:about="http://purl.obolibrary.org/obo/GAZ_00253881">
        <obo:RO_0001025 rdf:resource="http://purl.obolibrary.org/obo/GAZ_00051597"/>
        <obo:IAO_0000115>One of the Engineer Islands.</obo:IAO_0000115>
        <oboInOwl:hasOBONamespace>GAZ</oboInOwl:hasOBONamespace>
        <oboInOwl:id>GAZ:00253881</oboInOwl:id>
        <rdfs:label>Button Island</rdfs:label>
    </owl:NamedIndividual>
    


    <!-- http://purl.obolibrary.org/obo/GAZ_00253882 -->

    <owl:NamedIndividual rdf:about="http://purl.obolibrary.org/obo/GAZ_00253882">
        <obo:RO_0001025 rdf:resource="http://purl.obolibrary.org/obo/GAZ_00051597"/>
        <obo:IAO_0000115>One of the Engineer Islands.</obo:IAO_0000115>
        <oboInOwl:hasOBONamespace>GAZ</oboInOwl:hasOBONamespace>
        <oboInOwl:id>GAZ:00253882</oboInOwl:id>
        <rdfs:label>Bright Island</rdfs:label>
    </owl:NamedIndividual>
    


    <!-- http://purl.obolibrary.org/obo/GAZ_00253883 -->

    <owl:NamedIndividual rdf:about="http://purl.obolibrary.org/obo/GAZ_00253883">
        <obo:RO_0001025 rdf:resource="http://purl.obolibrary.org/obo/GAZ_00051597"/>
        <obo:IAO_0000115>One of the Engineer Islands.</obo:IAO_0000115>
        <oboInOwl:hasOBONamespace>GAZ</oboInOwl:hasOBONamespace>
        <oboInOwl:id>GAZ:00253883</oboInOwl:id>
        <rdfs:label>Powell Island</rdfs:label>
    </owl:NamedIndividual>
    


    <!-- http://purl.obolibrary.org/obo/GAZ_00253884 -->

    <owl:NamedIndividual rdf:about="http://purl.obolibrary.org/obo/GAZ_00253884">
        <obo:RO_0001025 rdf:resource="http://purl.obolibrary.org/obo/GAZ_00051597"/>
        <obo:IAO_0000115>One of the Engineer Islands.</obo:IAO_0000115>
        <oboInOwl:hasOBONamespace>GAZ</oboInOwl:hasOBONamespace>
        <oboInOwl:id>GAZ:00253884</oboInOwl:id>
        <rdfs:label>Pender Island</rdfs:label>
    </owl:NamedIndividual>
    


    <!-- http://purl.obolibrary.org/obo/GAZ_00253885 -->

    <owl:NamedIndividual rdf:about="http://purl.obolibrary.org/obo/GAZ_00253885">
        <obo:RO_0001025 rdf:resource="http://purl.obolibrary.org/obo/GAZ_00051597"/>
        <obo:IAO_0000115>One of the Engineer Islands.</obo:IAO_0000115>
        <oboInOwl:hasOBONamespace>GAZ</oboInOwl:hasOBONamespace>
        <oboInOwl:id>GAZ:00253885</oboInOwl:id>
        <rdfs:label>Messum Island</rdfs:label>
    </owl:NamedIndividual>
    


    <!-- http://purl.obolibrary.org/obo/GAZ_00253886 -->

    <owl:NamedIndividual rdf:about="http://purl.obolibrary.org/obo/GAZ_00253886">
        <obo:RO_0001025 rdf:resource="http://purl.obolibrary.org/obo/GAZ_00051597"/>
        <obo:IAO_0000115>One of the Engineer Islands.</obo:IAO_0000115>
        <oboInOwl:hasOBONamespace>GAZ</oboInOwl:hasOBONamespace>
        <oboInOwl:id>GAZ:00253886</oboInOwl:id>
        <rdfs:label>Good Island</rdfs:label>
    </owl:NamedIndividual>
    


    <!-- http://purl.obolibrary.org/obo/GAZ_00253887 -->

    <owl:NamedIndividual rdf:about="http://purl.obolibrary.org/obo/GAZ_00253887">
        <obo:RO_0001025 rdf:resource="http://purl.obolibrary.org/obo/GAZ_00051597"/>
        <obo:IAO_0000115>One of the Engineer Islands.</obo:IAO_0000115>
        <oboInOwl:hasOBONamespace>GAZ</oboInOwl:hasOBONamespace>
        <oboInOwl:id>GAZ:00253887</oboInOwl:id>
        <rdfs:label>Deeds Island</rdfs:label>
    </owl:NamedIndividual>
    


    <!-- http://purl.obolibrary.org/obo/GAZ_00253888 -->

    <owl:NamedIndividual rdf:about="http://purl.obolibrary.org/obo/GAZ_00253888">
        <obo:RO_0001025 rdf:resource="http://purl.obolibrary.org/obo/GAZ_00051597"/>
        <obo:IAO_0000115>One of the Engineer Islands.</obo:IAO_0000115>
        <oboInOwl:hasOBONamespace>GAZ</oboInOwl:hasOBONamespace>
        <oboInOwl:id>GAZ:00253888</oboInOwl:id>
        <rdfs:label>Flat Island</rdfs:label>
    </owl:NamedIndividual>
    


    <!-- http://purl.obolibrary.org/obo/GAZ_00253892 -->

    <owl:NamedIndividual rdf:about="http://purl.obolibrary.org/obo/GAZ_00253892">
        <obo:RO_0001025 rdf:resource="http://purl.obolibrary.org/obo/GAZ_00007255"/>
        <obo:IAO_0000115>A protected area. Located on the coast S of the Huon Peninsula.</obo:IAO_0000115>
        <oboInOwl:hasOBONamespace>GAZ</oboInOwl:hasOBONamespace>
        <oboInOwl:id>GAZ:00253892</oboInOwl:id>
        <rdfs:label>Karniali Wildlife Management Area</rdfs:label>
    </owl:NamedIndividual>
    


    <!-- http://purl.obolibrary.org/obo/GAZ_00253893 -->

    <owl:NamedIndividual rdf:about="http://purl.obolibrary.org/obo/GAZ_00253893">
        <obo:RO_0001025 rdf:resource="http://purl.obolibrary.org/obo/GAZ_00005198"/>
        <obo:IAO_0000115>An island.</obo:IAO_0000115>
        <oboInOwl:hasOBONamespace>GAZ</oboInOwl:hasOBONamespace>
        <oboInOwl:id>GAZ:00253893</oboInOwl:id>
        <rdfs:label>Sinup Island</rdfs:label>
    </owl:NamedIndividual>
    


    <!-- http://purl.obolibrary.org/obo/GAZ_00253894 -->

    <owl:NamedIndividual rdf:about="http://purl.obolibrary.org/obo/GAZ_00253894">
        <obo:RO_0001025 rdf:resource="http://purl.obolibrary.org/obo/GAZ_00253893"/>
        <obo:IAO_0000115>A protected area.</obo:IAO_0000115>
        <oboInOwl:hasOBONamespace>GAZ</oboInOwl:hasOBONamespace>
        <oboInOwl:id>GAZ:00253894</oboInOwl:id>
        <rdfs:label>Sinub Island Wildlife Management Area</rdfs:label>
    </owl:NamedIndividual>
    


    <!-- http://purl.obolibrary.org/obo/GAZ_00253895 -->

    <owl:NamedIndividual rdf:about="http://purl.obolibrary.org/obo/GAZ_00253895">
        <obo:RO_0001025 rdf:resource="http://purl.obolibrary.org/obo/GAZ_00005198"/>
        <obo:IAO_0000115>A protected area.</obo:IAO_0000115>
        <oboInOwl:hasOBONamespace>GAZ</oboInOwl:hasOBONamespace>
        <oboInOwl:id>GAZ:00253895</oboInOwl:id>
        <rdfs:label>Simbine Coast Wildlife Management Area</rdfs:label>
    </owl:NamedIndividual>
    


    <!-- http://purl.obolibrary.org/obo/GAZ_00253896 -->

    <owl:NamedIndividual rdf:about="http://purl.obolibrary.org/obo/GAZ_00253896">
        <obo:RO_0001025 rdf:resource="http://purl.obolibrary.org/obo/GAZ_00005266"/>
        <obo:IAO_0000115>A protected area. Established 1973.</obo:IAO_0000115>
        <oboInOwl:hasOBONamespace>GAZ</oboInOwl:hasOBONamespace>
        <oboInOwl:id>GAZ:00253896</oboInOwl:id>
        <rdfs:label>Cape Wom International Memorial Park</rdfs:label>
    </owl:NamedIndividual>
    


    <!-- http://purl.obolibrary.org/obo/GAZ_00253897 -->

    <owl:NamedIndividual rdf:about="http://purl.obolibrary.org/obo/GAZ_00253897">
        <obo:RO_0001025 rdf:resource="http://purl.obolibrary.org/obo/GAZ_00053882"/>
        <obo:IAO_0000115>A protected area. Established 1977.</obo:IAO_0000115>
        <oboInOwl:hasOBONamespace>GAZ</oboInOwl:hasOBONamespace>
        <oboInOwl:id>GAZ:00253897</oboInOwl:id>
        <rdfs:label>Randa Wildlife Management Area</rdfs:label>
    </owl:NamedIndividual>
    


    <!-- http://purl.obolibrary.org/obo/GAZ_00253898 -->

    <owl:NamedIndividual rdf:about="http://purl.obolibrary.org/obo/GAZ_00253898">
        <obo:RO_0001025 rdf:resource="http://purl.obolibrary.org/obo/GAZ_00053882"/>
        <obo:IAO_0000115>A protected area. Established 1977.</obo:IAO_0000115>
        <oboInOwl:hasOBONamespace>GAZ</oboInOwl:hasOBONamespace>
        <oboInOwl:id>GAZ:00253898</oboInOwl:id>
        <rdfs:label>Ranba Fauna Sanctuary</rdfs:label>
    </owl:NamedIndividual>
    


    <!-- http://purl.obolibrary.org/obo/GAZ_00253899 -->

    <owl:NamedIndividual rdf:about="http://purl.obolibrary.org/obo/GAZ_00253899">
        <obo:RO_0001025 rdf:resource="http://purl.obolibrary.org/obo/GAZ_00005198"/>
        <obo:IAO_0000115>An island. Located NW of Long Island.</obo:IAO_0000115>
        <oboInOwl:hasOBONamespace>GAZ</oboInOwl:hasOBONamespace>
        <oboInOwl:id>GAZ:00253899</oboInOwl:id>
        <rdfs:label>Crown Island</rdfs:label>
    </owl:NamedIndividual>
    


    <!-- http://purl.obolibrary.org/obo/GAZ_00253900 -->

    <owl:NamedIndividual rdf:about="http://purl.obolibrary.org/obo/GAZ_00253900">
        <obo:RO_0001025 rdf:resource="http://purl.obolibrary.org/obo/GAZ_00253899"/>
        <obo:IAO_0000115>A protected area. Established 1977.</obo:IAO_0000115>
        <oboInOwl:hasOBONamespace>GAZ</oboInOwl:hasOBONamespace>
        <oboInOwl:id>GAZ:00253900</oboInOwl:id>
        <rdfs:label>Crown Island Wildlife Management Area</rdfs:label>
    </owl:NamedIndividual>
    


    <!-- http://purl.obolibrary.org/obo/GAZ_00253902 -->

    <owl:NamedIndividual rdf:about="http://purl.obolibrary.org/obo/GAZ_00253902">
        <obo:RO_0001025 rdf:resource="http://purl.obolibrary.org/obo/GAZ_00005193"/>
        <obo:IAO_0000115>An island.</obo:IAO_0000115>
        <oboInOwl:hasOBONamespace>GAZ</oboInOwl:hasOBONamespace>
        <oboInOwl:id>GAZ:00253902</oboInOwl:id>
        <rdfs:label>Tuale Island</rdfs:label>
    </owl:NamedIndividual>
    


    <!-- http://purl.obolibrary.org/obo/GAZ_00253903 -->

    <owl:NamedIndividual rdf:about="http://purl.obolibrary.org/obo/GAZ_00253903">
        <obo:RO_0001025 rdf:resource="http://purl.obolibrary.org/obo/GAZ_00005193"/>
        <obo:IAO_0000115>An island.</obo:IAO_0000115>
        <oboInOwl:hasOBONamespace>GAZ</oboInOwl:hasOBONamespace>
        <oboInOwl:id>GAZ:00253903</oboInOwl:id>
        <rdfs:label>Mangamenek Island</rdfs:label>
    </owl:NamedIndividual>
    


    <!-- http://purl.obolibrary.org/obo/GAZ_00253904 -->

    <owl:NamedIndividual rdf:about="http://purl.obolibrary.org/obo/GAZ_00253904">
        <obo:RO_0001025 rdf:resource="http://purl.obolibrary.org/obo/GAZ_00007200"/>
        <obo:IAO_0000115>A narrow atoll formation of 35 km in length, orientated southeast-northwest; typical widths across the atoll lie in the range of 3-8 km.</obo:IAO_0000115>
        <oboInOwl:hasOBONamespace>GAZ</oboInOwl:hasOBONamespace>
        <oboInOwl:id>GAZ:00253904</oboInOwl:id>
        <rdfs:label>Nuguria Atoll</rdfs:label>
    </owl:NamedIndividual>
    


    <!-- http://purl.obolibrary.org/obo/GAZ_00253905 -->

    <owl:NamedIndividual rdf:about="http://purl.obolibrary.org/obo/GAZ_00253905">
        <obo:RO_0001025 rdf:resource="http://purl.obolibrary.org/obo/GAZ_00007200"/>
        <obo:IAO_0000115>An atoll. The smaller of the two atolls that comprise the Nuguria Islands grouping; it lies 4 km northwest from Nuguria atoll.</obo:IAO_0000115>
        <oboInOwl:hasOBONamespace>GAZ</oboInOwl:hasOBONamespace>
        <oboInOwl:id>GAZ:00253905</oboInOwl:id>
        <rdfs:label>Malum Atoll</rdfs:label>
    </owl:NamedIndividual>
    


    <!-- http://purl.obolibrary.org/obo/GAZ_00253906 -->

    <owl:NamedIndividual rdf:about="http://purl.obolibrary.org/obo/GAZ_00253906">
        <obo:RO_0001025 rdf:resource="http://purl.obolibrary.org/obo/GAZ_00016831"/>
        <obo:IAO_0000115>A caldera.</obo:IAO_0000115>
        <oboInOwl:hasOBONamespace>GAZ</oboInOwl:hasOBONamespace>
        <oboInOwl:id>GAZ:00253906</oboInOwl:id>
        <rdfs:label>Luise Caldera</rdfs:label>
    </owl:NamedIndividual>
    


    <!-- http://purl.obolibrary.org/obo/GAZ_00253907 -->

    <owl:NamedIndividual rdf:about="http://purl.obolibrary.org/obo/GAZ_00253907">
        <obo:RO_0001025 rdf:resource="http://purl.obolibrary.org/obo/GAZ_00016837"/>
        <obo:IAO_0000115>An island.</obo:IAO_0000115>
        <oboInOwl:hasOBONamespace>GAZ</oboInOwl:hasOBONamespace>
        <oboInOwl:id>GAZ:00253907</oboInOwl:id>
        <rdfs:label>Boang Island</rdfs:label>
    </owl:NamedIndividual>
    


    <!-- http://purl.obolibrary.org/obo/GAZ_00253908 -->

    <owl:NamedIndividual rdf:about="http://purl.obolibrary.org/obo/GAZ_00253908">
        <obo:RO_0001025 rdf:resource="http://purl.obolibrary.org/obo/GAZ_00007179"/>
        <obo:IAO_0000115>Islands located in the northwestern regions of the Bismarck Sea situated 23 km south from Manus and 21 km west from Lou. Less than 2 km to the northwest are the reefs of the Stuart Bank.</obo:IAO_0000115>
        <oboInOwl:hasOBONamespace>GAZ</oboInOwl:hasOBONamespace>
        <oboInOwl:id>GAZ:00253908</oboInOwl:id>
        <rdfs:label>Johnston Islands</rdfs:label>
    </owl:NamedIndividual>
    


    <!-- http://purl.obolibrary.org/obo/GAZ_00253909 -->

    <owl:NamedIndividual rdf:about="http://purl.obolibrary.org/obo/GAZ_00253909">
        <obo:RO_0001025 rdf:resource="http://purl.obolibrary.org/obo/GAZ_00253908"/>
        <obo:IAO_0000115>The largest of the Johnston Islands.</obo:IAO_0000115>
        <oboInOwl:hasOBONamespace>GAZ</oboInOwl:hasOBONamespace>
        <oboInOwl:id>GAZ:00253909</oboInOwl:id>
        <rdfs:label>Johnston Island</rdfs:label>
    </owl:NamedIndividual>
    


    <!-- http://purl.obolibrary.org/obo/GAZ_00253910 -->

    <owl:NamedIndividual rdf:about="http://purl.obolibrary.org/obo/GAZ_00253910">
        <obo:RO_0001025 rdf:resource="http://purl.obolibrary.org/obo/GAZ_00007179"/>
        <obo:IAO_0000115>Islands situated within the Saint Andrew Strait region 4 km northeast from Baluan and 5 km southwest from the Saint Andrew Islands; the island of Lou (the largest island in the region) is located 6 km to the north.</obo:IAO_0000115>
        <oboInOwl:hasOBONamespace>GAZ</oboInOwl:hasOBONamespace>
        <oboInOwl:id>GAZ:00253910</oboInOwl:id>
        <rdfs:label>Pam Islands</rdfs:label>
    </owl:NamedIndividual>
    


    <!-- http://purl.obolibrary.org/obo/GAZ_00253911 -->

    <owl:NamedIndividual rdf:about="http://purl.obolibrary.org/obo/GAZ_00253911">
        <obo:RO_0001025 rdf:resource="http://purl.obolibrary.org/obo/GAZ_00253910"/>
        <obo:IAO_0000115>An island on the SW of the Pam reef.</obo:IAO_0000115>
        <oboInOwl:hasOBONamespace>GAZ</oboInOwl:hasOBONamespace>
        <oboInOwl:id>GAZ:00253911</oboInOwl:id>
        <rdfs:label>Pam Mandian</rdfs:label>
    </owl:NamedIndividual>
    


    <!-- http://purl.obolibrary.org/obo/GAZ_00253912 -->

    <owl:NamedIndividual rdf:about="http://purl.obolibrary.org/obo/GAZ_00253912">
        <obo:RO_0001025 rdf:resource="http://purl.obolibrary.org/obo/GAZ_00253910"/>
        <obo:IAO_0000115>An island on the N of the Pam reef.</obo:IAO_0000115>
        <oboInOwl:hasOBONamespace>GAZ</oboInOwl:hasOBONamespace>
        <oboInOwl:id>GAZ:00253912</oboInOwl:id>
        <rdfs:label>Pam Lin</rdfs:label>
    </owl:NamedIndividual>
    


    <!-- http://purl.obolibrary.org/obo/GAZ_00253913 -->

    <owl:NamedIndividual rdf:about="http://purl.obolibrary.org/obo/GAZ_00253913">
        <obo:RO_0001025 rdf:resource="http://purl.obolibrary.org/obo/GAZ_00007179"/>
        <obo:IAO_0000115>A volcanic island group that lies within the northwestern reaches of the Bismarck Sea, 34 km southwest from the large island of Manus and 25 km west from Rambutyo; Lou lies 7 km to the west.</obo:IAO_0000115>
        <oboInOwl:hasOBONamespace>GAZ</oboInOwl:hasOBONamespace>
        <oboInOwl:id>GAZ:00253913</oboInOwl:id>
        <rdfs:label>Fedarb Islands</rdfs:label>
    </owl:NamedIndividual>
    


    <!-- http://purl.obolibrary.org/obo/GAZ_00253914 -->

    <owl:NamedIndividual rdf:about="http://purl.obolibrary.org/obo/GAZ_00253914">
        <obo:RO_0001025 rdf:resource="http://purl.obolibrary.org/obo/GAZ_00253913"/>
        <obo:IAO_0000115>One of the Fedarb Islands.</obo:IAO_0000115>
        <oboInOwl:hasOBONamespace>GAZ</oboInOwl:hasOBONamespace>
        <oboInOwl:id>GAZ:00253914</oboInOwl:id>
        <rdfs:label>Sivisa Island</rdfs:label>
    </owl:NamedIndividual>
    


    <!-- http://purl.obolibrary.org/obo/GAZ_00253915 -->

    <owl:NamedIndividual rdf:about="http://purl.obolibrary.org/obo/GAZ_00253915">
        <obo:RO_0001025 rdf:resource="http://purl.obolibrary.org/obo/GAZ_00253913"/>
        <obo:IAO_0000115>One of the Fedarb Islands.</obo:IAO_0000115>
        <oboInOwl:hasOBONamespace>GAZ</oboInOwl:hasOBONamespace>
        <oboInOwl:id>GAZ:00253915</oboInOwl:id>
        <rdfs:label>Small Sivisa Island</rdfs:label>
    </owl:NamedIndividual>
    


    <!-- http://purl.obolibrary.org/obo/GAZ_00253916 -->

    <owl:NamedIndividual rdf:about="http://purl.obolibrary.org/obo/GAZ_00253916">
        <obo:RO_0001025 rdf:resource="http://purl.obolibrary.org/obo/GAZ_00253913"/>
        <obo:IAO_0000115>One of the Fedarb Islands.</obo:IAO_0000115>
        <oboInOwl:hasOBONamespace>GAZ</oboInOwl:hasOBONamespace>
        <oboInOwl:id>GAZ:00253916</oboInOwl:id>
        <rdfs:label>Chokua Island</rdfs:label>
    </owl:NamedIndividual>
    


    <!-- http://purl.obolibrary.org/obo/GAZ_00253917 -->

    <owl:NamedIndividual rdf:about="http://purl.obolibrary.org/obo/GAZ_00253917">
        <obo:RO_0001025 rdf:resource="http://purl.obolibrary.org/obo/GAZ_00253913"/>
        <obo:IAO_0000115>One of the Fedarb Islands.</obo:IAO_0000115>
        <oboInOwl:hasOBONamespace>GAZ</oboInOwl:hasOBONamespace>
        <oboInOwl:id>GAZ:00253917</oboInOwl:id>
        <rdfs:label>Lolau Island</rdfs:label>
    </owl:NamedIndividual>
    


    <!-- http://purl.obolibrary.org/obo/GAZ_00253918 -->

    <owl:NamedIndividual rdf:about="http://purl.obolibrary.org/obo/GAZ_00253918">
        <obo:RO_0001025 rdf:resource="http://purl.obolibrary.org/obo/GAZ_00005191"/>
        <obo:IAO_0000115>A protected area.</obo:IAO_0000115>
        <oboInOwl:hasOBONamespace>GAZ</oboInOwl:hasOBONamespace>
        <oboInOwl:id>GAZ:00253918</oboInOwl:id>
        <rdfs:label>Kimbe Bay Marine Conservation Area</rdfs:label>
    </owl:NamedIndividual>
    


    <!-- http://purl.obolibrary.org/obo/GAZ_00253919 -->

    <owl:NamedIndividual rdf:about="http://purl.obolibrary.org/obo/GAZ_00253919">
        <obo:RO_0001025 rdf:resource="http://purl.obolibrary.org/obo/GAZ_00005191"/>
        <obo:IAO_0000115>A protected area. Established 1976.</obo:IAO_0000115>
        <oboInOwl:hasOBONamespace>GAZ</oboInOwl:hasOBONamespace>
        <oboInOwl:id>GAZ:00253919</oboInOwl:id>
        <rdfs:label>Garu Wildlife Management Area</rdfs:label>
    </owl:NamedIndividual>
    


    <!-- http://purl.obolibrary.org/obo/GAZ_00253920 -->

    <owl:NamedIndividual rdf:about="http://purl.obolibrary.org/obo/GAZ_00253920">
        <obo:RO_0001025 rdf:resource="http://purl.obolibrary.org/obo/GAZ_00005192"/>
        <obo:IAO_0000115>A protected area. Established 1973.</obo:IAO_0000115>
        <oboInOwl:hasOBONamespace>GAZ</oboInOwl:hasOBONamespace>
        <oboInOwl:id>GAZ:00253920</oboInOwl:id>
        <rdfs:label>Talele Islands Nature Reserve and Provincial Park</rdfs:label>
    </owl:NamedIndividual>
    


    <!-- http://purl.obolibrary.org/obo/GAZ_00253921 -->

    <owl:NamedIndividual rdf:about="http://purl.obolibrary.org/obo/GAZ_00253921">
        <obo:RO_0001025 rdf:resource="http://purl.obolibrary.org/obo/GAZ_00253920"/>
        <obo:IAO_0000115>Eight coralline islands.</obo:IAO_0000115>
        <oboInOwl:hasOBONamespace>GAZ</oboInOwl:hasOBONamespace>
        <oboInOwl:id>GAZ:00253921</oboInOwl:id>
        <rdfs:label>Talele Islands</rdfs:label>
    </owl:NamedIndividual>
    


    <!-- http://purl.obolibrary.org/obo/GAZ_00253922 -->

    <owl:NamedIndividual rdf:about="http://purl.obolibrary.org/obo/GAZ_00253922">
        <obo:RO_0001025 rdf:resource="http://purl.obolibrary.org/obo/GAZ_00253923"/>
        <obo:IAO_0000115>A protected area. Established 1973-01-01.</obo:IAO_0000115>
        <oboInOwl:hasOBONamespace>GAZ</oboInOwl:hasOBONamespace>
        <oboInOwl:id>GAZ:00253922</oboInOwl:id>
        <rdfs:label>Nanuk Island Provincial Park</rdfs:label>
    </owl:NamedIndividual>
    


    <!-- http://purl.obolibrary.org/obo/GAZ_00253923 -->

    <owl:NamedIndividual rdf:about="http://purl.obolibrary.org/obo/GAZ_00253923">
        <obo:RO_0001025 rdf:resource="http://purl.obolibrary.org/obo/GAZ_00005192"/>
        <obo:IAO_0000115>A low coralline island.</obo:IAO_0000115>
        <oboInOwl:hasOBONamespace>GAZ</oboInOwl:hasOBONamespace>
        <oboInOwl:id>GAZ:00253923</oboInOwl:id>
        <rdfs:label>Nanuk Island</rdfs:label>
    </owl:NamedIndividual>
    


    <!-- http://purl.obolibrary.org/obo/GAZ_00253924 -->

    <owl:NamedIndividual rdf:about="http://purl.obolibrary.org/obo/GAZ_00253924">
        <obo:RO_0001025 rdf:resource="http://purl.obolibrary.org/obo/GAZ_00016821"/>
        <obo:IAO_0000115>One of the Purdy Islands.</obo:IAO_0000115>
        <oboInOwl:hasOBONamespace>GAZ</oboInOwl:hasOBONamespace>
        <oboInOwl:id>GAZ:00253924</oboInOwl:id>
        <rdfs:label>Mole Island</rdfs:label>
    </owl:NamedIndividual>
    


    <!-- http://purl.obolibrary.org/obo/GAZ_00253925 -->

    <owl:NamedIndividual rdf:about="http://purl.obolibrary.org/obo/GAZ_00253925">
        <obo:RO_0001025 rdf:resource="http://purl.obolibrary.org/obo/GAZ_00016821"/>
        <obo:IAO_0000115>One of the Purdy Islands.</obo:IAO_0000115>
        <oboInOwl:hasOBONamespace>GAZ</oboInOwl:hasOBONamespace>
        <oboInOwl:id>GAZ:00253925</oboInOwl:id>
        <rdfs:label>Mouse Island</rdfs:label>
    </owl:NamedIndividual>
    


    <!-- http://purl.obolibrary.org/obo/GAZ_00253926 -->

    <owl:NamedIndividual rdf:about="http://purl.obolibrary.org/obo/GAZ_00253926">
        <obo:RO_0001025 rdf:resource="http://purl.obolibrary.org/obo/GAZ_00016821"/>
        <obo:IAO_0000115>One of the Purdy Islands.</obo:IAO_0000115>
        <oboInOwl:hasOBONamespace>GAZ</oboInOwl:hasOBONamespace>
        <oboInOwl:id>GAZ:00253926</oboInOwl:id>
        <rdfs:label>Rat Island</rdfs:label>
    </owl:NamedIndividual>
    


    <!-- http://purl.obolibrary.org/obo/GAZ_00253927 -->

    <owl:NamedIndividual rdf:about="http://purl.obolibrary.org/obo/GAZ_00253927">
        <obo:RO_0001025 rdf:resource="http://purl.obolibrary.org/obo/GAZ_00016821"/>
        <obo:IAO_0000115>Two small islands.</obo:IAO_0000115>
        <oboInOwl:hasOBONamespace>GAZ</oboInOwl:hasOBONamespace>
        <oboInOwl:id>GAZ:00253927</oboInOwl:id>
        <rdfs:label>Bat Islands</rdfs:label>
    </owl:NamedIndividual>
    


    <!-- http://purl.obolibrary.org/obo/GAZ_00253928 -->

    <owl:NamedIndividual rdf:about="http://purl.obolibrary.org/obo/GAZ_00253928">
        <obo:RO_0001025 rdf:resource="http://purl.obolibrary.org/obo/GAZ_00051649"/>
        <obo:IAO_0000115>A 34 km long by 18 km wide atoll open on its western side.</obo:IAO_0000115>
        <oboInOwl:hasOBONamespace>GAZ</oboInOwl:hasOBONamespace>
        <oboInOwl:id>GAZ:00253928</oboInOwl:id>
        <rdfs:label>Ninigo Group</rdfs:label>
    </owl:NamedIndividual>
    


    <!-- http://purl.obolibrary.org/obo/GAZ_00253929 -->

    <owl:NamedIndividual rdf:about="http://purl.obolibrary.org/obo/GAZ_00253929">
        <obo:RO_0001025 rdf:resource="http://purl.obolibrary.org/obo/GAZ_00051655"/>
        <obo:IAO_0000115>An island on Liot Atoll.</obo:IAO_0000115>
        <oboInOwl:hasOBONamespace>GAZ</oboInOwl:hasOBONamespace>
        <oboInOwl:id>GAZ:00253929</oboInOwl:id>
        <rdfs:label>Ufe Island</rdfs:label>
    </owl:NamedIndividual>
    


    <!-- http://purl.obolibrary.org/obo/GAZ_00253931 -->

    <owl:NamedIndividual rdf:about="http://purl.obolibrary.org/obo/GAZ_00253931">
        <obo:RO_0001025 rdf:resource="http://purl.obolibrary.org/obo/GAZ_00253932"/>
        <obo:IAO_0000115>A protected area. Established 1998.</obo:IAO_0000115>
        <oboInOwl:hasOBONamespace>GAZ</oboInOwl:hasOBONamespace>
        <oboInOwl:id>GAZ:00253931</oboInOwl:id>
        <rdfs:label>East Hunstein Reserve</rdfs:label>
    </owl:NamedIndividual>
    


    <!-- http://purl.obolibrary.org/obo/GAZ_00253932 -->

    <owl:NamedIndividual rdf:about="http://purl.obolibrary.org/obo/GAZ_00253932">
        <obo:RO_0001025 rdf:resource="http://purl.obolibrary.org/obo/GAZ_00005266"/>
        <obo:IAO_0000115>A mountain range.</obo:IAO_0000115>
        <oboInOwl:hasOBONamespace>GAZ</oboInOwl:hasOBONamespace>
        <oboInOwl:id>GAZ:00253932</oboInOwl:id>
        <rdfs:label>Hunstein Range</rdfs:label>
    </owl:NamedIndividual>
    


    <!-- http://purl.obolibrary.org/obo/GAZ_00253933 -->

    <owl:NamedIndividual rdf:about="http://purl.obolibrary.org/obo/GAZ_00253933">
        <obo:RO_0001025 rdf:resource="http://purl.obolibrary.org/obo/GAZ_00012659"/>
        <obo:IAO_0000115>A protected area. Established 1987.</obo:IAO_0000115>
        <oboInOwl:hasOBONamespace>GAZ</oboInOwl:hasOBONamespace>
        <oboInOwl:id>GAZ:00253933</oboInOwl:id>
        <rdfs:label>Neiru Wildlife Management Area</rdfs:label>
    </owl:NamedIndividual>
    


    <!-- http://purl.obolibrary.org/obo/GAZ_00253934 -->

    <owl:NamedIndividual rdf:about="http://purl.obolibrary.org/obo/GAZ_00253934">
        <obo:RO_0001025 rdf:resource="http://purl.obolibrary.org/obo/GAZ_00012661"/>
        <obo:IAO_0000115>A protected area. Established 1968.</obo:IAO_0000115>
        <oboInOwl:hasOBONamespace>GAZ</oboInOwl:hasOBONamespace>
        <oboInOwl:id>GAZ:00253934</oboInOwl:id>
        <rdfs:label>Baiyer River Sanctuary</rdfs:label>
    </owl:NamedIndividual>
    


    <!-- http://purl.obolibrary.org/obo/GAZ_00253935 -->

    <owl:NamedIndividual rdf:about="http://purl.obolibrary.org/obo/GAZ_00253935">
        <obo:RO_0001025 rdf:resource="http://purl.obolibrary.org/obo/GAZ_00012664"/>
        <obo:IAO_0000115>A protected area.</obo:IAO_0000115>
        <oboInOwl:hasOBONamespace>GAZ</oboInOwl:hasOBONamespace>
        <oboInOwl:id>GAZ:00253935</oboInOwl:id>
        <rdfs:label>Bosavi Wildlife Reserve</rdfs:label>
    </owl:NamedIndividual>
    


    <!-- http://purl.obolibrary.org/obo/GAZ_00253936 -->

    <owl:NamedIndividual rdf:about="http://purl.obolibrary.org/obo/GAZ_00253936">
        <obo:RO_0001025 rdf:resource="http://purl.obolibrary.org/obo/GAZ_00012657"/>
        <obo:IAO_0000115>A protected area. Established 1987.</obo:IAO_0000115>
        <oboInOwl:hasOBONamespace>GAZ</oboInOwl:hasOBONamespace>
        <oboInOwl:id>GAZ:00253936</oboInOwl:id>
        <rdfs:label>Iomare Wildlife Management Area</rdfs:label>
    </owl:NamedIndividual>
    


    <!-- http://purl.obolibrary.org/obo/GAZ_00253937 -->

    <owl:NamedIndividual rdf:about="http://purl.obolibrary.org/obo/GAZ_00253937">
        <obo:RO_0001025 rdf:resource="http://purl.obolibrary.org/obo/GAZ_00012659"/>
        <obo:IAO_0000115>A protected area.</obo:IAO_0000115>
        <oboInOwl:hasOBONamespace>GAZ</oboInOwl:hasOBONamespace>
        <oboInOwl:id>GAZ:00253937</oboInOwl:id>
        <rdfs:label>Lakekamu Basin Integrated Conservation and Development Project Area</rdfs:label>
    </owl:NamedIndividual>
    


    <!-- http://purl.obolibrary.org/obo/GAZ_00253938 -->

    <owl:NamedIndividual rdf:about="http://purl.obolibrary.org/obo/GAZ_00253938">
        <obo:RO_0001025 rdf:resource="http://purl.obolibrary.org/obo/GAZ_00253939"/>
        <obo:IAO_0000115>A protected area.</obo:IAO_0000115>
        <oboInOwl:hasOBONamespace>GAZ</oboInOwl:hasOBONamespace>
        <oboInOwl:id>GAZ:00253938</oboInOwl:id>
        <rdfs:label>Moitaka Wildlife Sanctuary</rdfs:label>
    </owl:NamedIndividual>
    


    <!-- http://purl.obolibrary.org/obo/GAZ_00253939 -->

    <owl:NamedIndividual rdf:about="http://purl.obolibrary.org/obo/GAZ_00253939">
        <obo:RO_0001025 rdf:resource="http://purl.obolibrary.org/obo/GAZ_00005264"/>
        <obo:IAO_0000115>An island.</obo:IAO_0000115>
        <oboInOwl:hasOBONamespace>GAZ</oboInOwl:hasOBONamespace>
        <oboInOwl:id>GAZ:00253939</oboInOwl:id>
        <rdfs:label>Henderson Island</rdfs:label>
    </owl:NamedIndividual>
    


    <!-- http://purl.obolibrary.org/obo/GAZ_00253940 -->

    <owl:NamedIndividual rdf:about="http://purl.obolibrary.org/obo/GAZ_00253940">
        <obo:RO_0001025 rdf:resource="http://purl.obolibrary.org/obo/GAZ_00012662"/>
        <obo:IAO_0000115>A protected area. Located on the NE coast, Collinwood Bay Area.</obo:IAO_0000115>
        <oboInOwl:hasOBONamespace>GAZ</oboInOwl:hasOBONamespace>
        <oboInOwl:id>GAZ:00253940</oboInOwl:id>
        <rdfs:label>Maisin Integrated Conservation and Development Project Area</rdfs:label>
    </owl:NamedIndividual>
    


    <!-- http://purl.obolibrary.org/obo/GAZ_00253941 -->

    <owl:NamedIndividual rdf:about="http://purl.obolibrary.org/obo/GAZ_00253941">
        <obo:RO_0001025 rdf:resource="http://purl.obolibrary.org/obo/GAZ_00005264"/>
        <obo:IAO_0000115>A protected area. Located in Port Moresby. State land behind Parliament House.</obo:IAO_0000115>
        <oboInOwl:hasOBONamespace>GAZ</oboInOwl:hasOBONamespace>
        <oboInOwl:id>GAZ:00253941</oboInOwl:id>
        <rdfs:label>Waigani National Park</rdfs:label>
    </owl:NamedIndividual>
    


    <!-- http://purl.obolibrary.org/obo/GAZ_00253942 -->

    <owl:NamedIndividual rdf:about="http://purl.obolibrary.org/obo/GAZ_00253942">
        <obo:RO_0001025 rdf:resource="http://purl.obolibrary.org/obo/GAZ_00005198"/>
        <obo:IAO_0000115>A protected area. Established 1977.</obo:IAO_0000115>
        <oboInOwl:hasOBONamespace>GAZ</oboInOwl:hasOBONamespace>
        <oboInOwl:id>GAZ:00253942</oboInOwl:id>
        <rdfs:label>Balek Fauna Sanctuary</rdfs:label>
    </owl:NamedIndividual>
    


    <!-- http://purl.obolibrary.org/obo/GAZ_00253943 -->

    <owl:NamedIndividual rdf:about="http://purl.obolibrary.org/obo/GAZ_00253943">
        <obo:RO_0001025 rdf:resource="http://purl.obolibrary.org/obo/GAZ_00016855"/>
        <obo:IAO_0000115>A protected area. Established 1961.</obo:IAO_0000115>
        <oboInOwl:hasOBONamespace>GAZ</oboInOwl:hasOBONamespace>
        <oboInOwl:id>GAZ:00253943</oboInOwl:id>
        <rdfs:label>Lake Lavu Wildlife Management Area</rdfs:label>
    </owl:NamedIndividual>
    


    <!-- http://purl.obolibrary.org/obo/GAZ_00253945 -->

    <owl:NamedIndividual rdf:about="http://purl.obolibrary.org/obo/GAZ_00253945">
        <obo:RO_0001025 rdf:resource="http://purl.obolibrary.org/obo/GAZ_00012665"/>
        <obo:IAO_0000115>A protected area. Estabished 1986/1991.</obo:IAO_0000115>
        <oboInOwl:hasOBONamespace>GAZ</oboInOwl:hasOBONamespace>
        <oboInOwl:id>GAZ:00253945</oboInOwl:id>
        <rdfs:label>Jimi Valley National Park</rdfs:label>
    </owl:NamedIndividual>
    


    <!-- http://purl.obolibrary.org/obo/GAZ_00253946 -->

    <owl:NamedIndividual rdf:about="http://purl.obolibrary.org/obo/GAZ_00253946">
        <obo:RO_0001025 rdf:resource="http://purl.obolibrary.org/obo/GAZ_00005192"/>
        <obo:IAO_0000115>A protected area.</obo:IAO_0000115>
        <oboInOwl:hasOBONamespace>GAZ</oboInOwl:hasOBONamespace>
        <oboInOwl:id>GAZ:00253946</oboInOwl:id>
        <rdfs:label>Wide Bay Kamplur Conservation Area</rdfs:label>
    </owl:NamedIndividual>
    


    <!-- http://purl.obolibrary.org/obo/GAZ_00253947 -->

    <owl:NamedIndividual rdf:about="http://purl.obolibrary.org/obo/GAZ_00253947">
        <obo:RO_0001025 rdf:resource="http://purl.obolibrary.org/obo/GAZ_00005191"/>
        <obo:IAO_0000115>A protected area. Estabished 1991.</obo:IAO_0000115>
        <oboInOwl:hasOBONamespace>GAZ</oboInOwl:hasOBONamespace>
        <oboInOwl:id>GAZ:00253947</oboInOwl:id>
        <rdfs:label>Lorko National Park</rdfs:label>
    </owl:NamedIndividual>
    


    <!-- http://purl.obolibrary.org/obo/GAZ_00253948 -->

    <owl:NamedIndividual rdf:about="http://purl.obolibrary.org/obo/GAZ_00253948">
        <obo:RO_0001025 rdf:resource="http://purl.obolibrary.org/obo/GAZ_00022437"/>
        <obo:IAO_0000115>A protected area. Established 1977.</obo:IAO_0000115>
        <oboInOwl:hasOBONamespace>GAZ</oboInOwl:hasOBONamespace>
        <oboInOwl:id>GAZ:00253948</oboInOwl:id>
        <rdfs:label>Siwi Utame Wildlife Management Area</rdfs:label>
    </owl:NamedIndividual>
    


    <!-- http://purl.obolibrary.org/obo/GAZ_00253949 -->

    <owl:NamedIndividual rdf:about="http://purl.obolibrary.org/obo/GAZ_00253949">
        <obo:RO_0001025 rdf:resource="http://purl.obolibrary.org/obo/GAZ_00005191"/>
        <obo:IAO_0000115>A protected area. Established 1975.</obo:IAO_0000115>
        <oboInOwl:hasOBONamespace>GAZ</oboInOwl:hasOBONamespace>
        <oboInOwl:id>GAZ:00253949</oboInOwl:id>
        <rdfs:label>Pokili Wildlife Management Area</rdfs:label>
    </owl:NamedIndividual>
    


    <!-- http://purl.obolibrary.org/obo/GAZ_00253950 -->

    <owl:NamedIndividual rdf:about="http://purl.obolibrary.org/obo/GAZ_00253950">
        <obo:RO_0001025 rdf:resource="http://purl.obolibrary.org/obo/GAZ_00012657"/>
        <obo:IAO_0000115>A protected area. Located just outside Port Moresby. Established 1987.</obo:IAO_0000115>
        <oboInOwl:hasOBONamespace>GAZ</oboInOwl:hasOBONamespace>
        <oboInOwl:id>GAZ:00253950</oboInOwl:id>
        <rdfs:label>Paga Hill Scenic Reserve</rdfs:label>
    </owl:NamedIndividual>
    


    <!-- http://purl.obolibrary.org/obo/GAZ_00253951 -->

    <owl:NamedIndividual rdf:about="http://purl.obolibrary.org/obo/GAZ_00253951">
        <obo:RO_0001025 rdf:resource="http://purl.obolibrary.org/obo/GAZ_00005198"/>
        <obo:IAO_0000115>A protected area.</obo:IAO_0000115>
        <oboInOwl:hasOBONamespace>GAZ</oboInOwl:hasOBONamespace>
        <oboInOwl:id>GAZ:00253951</oboInOwl:id>
        <rdfs:label>Kau Wildlife Management Area</rdfs:label>
    </owl:NamedIndividual>
    


    <!-- http://purl.obolibrary.org/obo/GAZ_00253952 -->

    <owl:NamedIndividual rdf:about="http://purl.obolibrary.org/obo/GAZ_00253952">
        <obo:RO_0001025 rdf:resource="http://purl.obolibrary.org/obo/GAZ_00010064"/>
        <obo:IAO_0000115>A protected area. Encompasses alluvial Papuan Plain to slopes of Crater Mountain lowland rainforest of the Purari River on the Great Papuan Plain to Montane cloud forest on the slopes of Crater Mountain. Established 1994.</obo:IAO_0000115>
        <oboInOwl:hasOBONamespace>GAZ</oboInOwl:hasOBONamespace>
        <oboInOwl:id>GAZ:00253952</oboInOwl:id>
        <rdfs:label>Crater Mountain Wildlife Reserve</rdfs:label>
    </owl:NamedIndividual>
    


    <!-- http://purl.obolibrary.org/obo/GAZ_00253953 -->

    <owl:NamedIndividual rdf:about="http://purl.obolibrary.org/obo/GAZ_00253953">
        <obo:RO_0001025 rdf:resource="http://purl.obolibrary.org/obo/GAZ_00012658"/>
        <obo:IAO_0000115>A protected area. Established 1991.</obo:IAO_0000115>
        <oboInOwl:hasOBONamespace>GAZ</oboInOwl:hasOBONamespace>
        <oboInOwl:id>GAZ:00253953</oboInOwl:id>
        <rdfs:label>Mount Wilhelm National Park</rdfs:label>
    </owl:NamedIndividual>
    


    <!-- http://purl.obolibrary.org/obo/GAZ_00253954 -->

    <owl:NamedIndividual rdf:about="http://purl.obolibrary.org/obo/GAZ_00253954">
        <obo:RO_0001025 rdf:resource="http://purl.obolibrary.org/obo/GAZ_00250665"/>
        <obo:IAO_0000115>A protected area. Includes small area covering the escarpment rising at the top of the Song River. Established 1986.</obo:IAO_0000115>
        <oboInOwl:hasOBONamespace>GAZ</oboInOwl:hasOBONamespace>
        <oboInOwl:id>GAZ:00253954</oboInOwl:id>
        <rdfs:label>Mount Nuraseng Wildlife Management Area</rdfs:label>
    </owl:NamedIndividual>
    


    <!-- http://purl.obolibrary.org/obo/GAZ_00253955 -->

    <owl:NamedIndividual rdf:about="http://purl.obolibrary.org/obo/GAZ_00253955">
        <obo:RO_0001025 rdf:resource="http://purl.obolibrary.org/obo/GAZ_00012657"/>
        <obo:IAO_0000115>A protected area. Established 1981.</obo:IAO_0000115>
        <oboInOwl:hasOBONamespace>GAZ</oboInOwl:hasOBONamespace>
        <oboInOwl:id>GAZ:00253955</oboInOwl:id>
        <rdfs:label>Zo-oimaga Wildlife Management Area</rdfs:label>
    </owl:NamedIndividual>
    


    <!-- http://purl.obolibrary.org/obo/GAZ_00253956 -->

    <owl:NamedIndividual rdf:about="http://purl.obolibrary.org/obo/GAZ_00253956">
        <obo:RO_0001025 rdf:resource="http://purl.obolibrary.org/obo/GAZ_00007255"/>
        <obo:IAO_0000115>A protected area.</obo:IAO_0000115>
        <oboInOwl:hasOBONamespace>GAZ</oboInOwl:hasOBONamespace>
        <oboInOwl:id>GAZ:00253956</oboInOwl:id>
        <rdfs:label>Mount Susu National Park</rdfs:label>
    </owl:NamedIndividual>
    


    <!-- http://purl.obolibrary.org/obo/GAZ_00253957 -->

    <owl:NamedIndividual rdf:about="http://purl.obolibrary.org/obo/GAZ_00253957">
        <obo:RO_0001025 rdf:resource="http://purl.obolibrary.org/obo/GAZ_00007255"/>
        <obo:IAO_0000115>A protected area. Located near Bulolo. established 1962/1989.</obo:IAO_0000115>
        <oboInOwl:hasOBONamespace>GAZ</oboInOwl:hasOBONamespace>
        <oboInOwl:id>GAZ:00253957</oboInOwl:id>
        <rdfs:label>McAdams National Park</rdfs:label>
    </owl:NamedIndividual>
    


    <!-- http://purl.obolibrary.org/obo/GAZ_00253958 -->

    <owl:NamedIndividual rdf:about="http://purl.obolibrary.org/obo/GAZ_00253958">
        <obo:IAO_0000115>A protected area.</obo:IAO_0000115>
        <oboInOwl:hasOBONamespace>GAZ</oboInOwl:hasOBONamespace>
        <oboInOwl:id>GAZ:00253958</oboInOwl:id>
        <rdfs:label>Kokoda Trail National Park</rdfs:label>
    </owl:NamedIndividual>
    


    <!-- http://purl.obolibrary.org/obo/GAZ_00253959 -->

    <owl:NamedIndividual rdf:about="http://purl.obolibrary.org/obo/GAZ_00253959">
        <obo:RO_0001025 rdf:resource="http://purl.obolibrary.org/obo/GAZ_00253958"/>
        <obo:IAO_0000115>A single-file foot thoroughfare that runs 96 km overland through the Owen Stanley Range in Papua New Guinea. The track is between Owers Corner in Central Province, 50 km east of Port Moresby, and then crosses rugged and isolated terrain to the village of Kokoda in Northern Province.</obo:IAO_0000115>
        <oboInOwl:hasOBONamespace>GAZ</oboInOwl:hasOBONamespace>
        <oboInOwl:id>GAZ:00253959</oboInOwl:id>
        <rdfs:label>Kokoda Trail</rdfs:label>
    </owl:NamedIndividual>
    


    <!-- http://purl.obolibrary.org/obo/GAZ_00253960 -->

    <owl:NamedIndividual rdf:about="http://purl.obolibrary.org/obo/GAZ_00253960">
        <obo:RO_0001025 rdf:resource="http://purl.obolibrary.org/obo/GAZ_00005192"/>
        <obo:IAO_0000115>A protected area. Established 2003.</obo:IAO_0000115>
        <oboInOwl:hasOBONamespace>GAZ</oboInOwl:hasOBONamespace>
        <oboInOwl:id>GAZ:00253960</oboInOwl:id>
        <rdfs:label>Klampun Conservation Area</rdfs:label>
    </owl:NamedIndividual>
    


    <!-- http://purl.obolibrary.org/obo/GAZ_00253961 -->

    <owl:NamedIndividual rdf:about="http://purl.obolibrary.org/obo/GAZ_00253961">
        <obo:RO_0001025 rdf:resource="http://purl.obolibrary.org/obo/GAZ_00016831"/>
        <obo:IAO_0000115>A protected area. Established 1991.</obo:IAO_0000115>
        <oboInOwl:hasOBONamespace>GAZ</oboInOwl:hasOBONamespace>
        <oboInOwl:id>GAZ:00253961</oboInOwl:id>
        <rdfs:label>Lihir Island Fauna Protected Area</rdfs:label>
    </owl:NamedIndividual>
    


    <!-- http://purl.obolibrary.org/obo/GAZ_00253962 -->

    <owl:NamedIndividual rdf:about="http://purl.obolibrary.org/obo/GAZ_00253962">
        <obo:RO_0001025 rdf:resource="http://purl.obolibrary.org/obo/GAZ_00010064"/>
        <obo:IAO_0000115>A protected area. Located 11 km from Goroka, on a spur at Mount Otto in the Bismarck Range. Established 1989.</obo:IAO_0000115>
        <oboInOwl:hasOBONamespace>GAZ</oboInOwl:hasOBONamespace>
        <oboInOwl:id>GAZ:00253962</oboInOwl:id>
        <rdfs:label>Mount Gahavisuka Park</rdfs:label>
    </owl:NamedIndividual>
    


    <!-- http://purl.obolibrary.org/obo/GAZ_00253963 -->

    <owl:NamedIndividual rdf:about="http://purl.obolibrary.org/obo/GAZ_00253963">
        <obo:RO_0001025 rdf:resource="http://purl.obolibrary.org/obo/GAZ_00007255"/>
        <obo:IAO_0000115>A protected area. Located near Wau. Established 1990.</obo:IAO_0000115>
        <oboInOwl:hasOBONamespace>GAZ</oboInOwl:hasOBONamespace>
        <oboInOwl:id>GAZ:00253963</oboInOwl:id>
        <rdfs:label>Mount Kaindi Wildlife Management Area</rdfs:label>
    </owl:NamedIndividual>
    


    <!-- http://purl.obolibrary.org/obo/GAZ_00253964 -->

    <owl:NamedIndividual rdf:about="http://purl.obolibrary.org/obo/GAZ_00253964">
        <obo:RO_0001025 rdf:resource="http://purl.obolibrary.org/obo/GAZ_00012662"/>
        <obo:IAO_0000115>A protected area.</obo:IAO_0000115>
        <oboInOwl:hasOBONamespace>GAZ</oboInOwl:hasOBONamespace>
        <oboInOwl:id>GAZ:00253964</oboInOwl:id>
        <rdfs:label>Hombareta Wildlife Management Area</rdfs:label>
    </owl:NamedIndividual>
    


    <!-- http://purl.obolibrary.org/obo/GAZ_00253965 -->

    <owl:NamedIndividual rdf:about="http://purl.obolibrary.org/obo/GAZ_00253965">
        <obo:RO_0001025 rdf:resource="http://purl.obolibrary.org/obo/GAZ_00016856"/>
        <obo:IAO_0000115>A protected area.</obo:IAO_0000115>
        <oboInOwl:hasOBONamespace>GAZ</oboInOwl:hasOBONamespace>
        <oboInOwl:id>GAZ:00253965</oboInOwl:id>
        <rdfs:label>Normanby Islands Marine Park/Reserve</rdfs:label>
    </owl:NamedIndividual>
    


    <!-- http://purl.obolibrary.org/obo/GAZ_00253966 -->

    <owl:NamedIndividual rdf:about="http://purl.obolibrary.org/obo/GAZ_00253966">
        <obo:RO_0001025 rdf:resource="http://purl.obolibrary.org/obo/GAZ_00005182"/>
        <obo:IAO_0000115>A protected area. Extends 1km from the coast of Aroma, Kieta, Arawa. Loloko &amp; Toniva. Established 1990.</obo:IAO_0000115>
        <oboInOwl:hasOBONamespace>GAZ</oboInOwl:hasOBONamespace>
        <oboInOwl:id>GAZ:00253966</oboInOwl:id>
        <rdfs:label>Paring Wildlife Management Area</rdfs:label>
    </owl:NamedIndividual>
    


    <!-- http://purl.obolibrary.org/obo/GAZ_00253967 -->

    <owl:NamedIndividual rdf:about="http://purl.obolibrary.org/obo/GAZ_00253967">
        <obo:RO_0001025 rdf:resource="http://purl.obolibrary.org/obo/GAZ_00253969"/>
        <obo:IAO_0000115>An island.</obo:IAO_0000115>
        <oboInOwl:hasOBONamespace>GAZ</oboInOwl:hasOBONamespace>
        <oboInOwl:id>GAZ:00253967</oboInOwl:id>
        <rdfs:label>Tab Island</rdfs:label>
    </owl:NamedIndividual>
    


    <!-- http://purl.obolibrary.org/obo/GAZ_00253968 -->

    <owl:NamedIndividual rdf:about="http://purl.obolibrary.org/obo/GAZ_00253968">
        <obo:RO_0001025 rdf:resource="http://purl.obolibrary.org/obo/GAZ_00005198"/>
        <obo:IAO_0000115>A coastal lagoon.</obo:IAO_0000115>
        <oboInOwl:hasOBONamespace>GAZ</oboInOwl:hasOBONamespace>
        <oboInOwl:id>GAZ:00253968</oboInOwl:id>
        <rdfs:label>Madang Lagoon</rdfs:label>
    </owl:NamedIndividual>
    


    <!-- http://purl.obolibrary.org/obo/GAZ_00253969 -->

    <owl:NamedIndividual rdf:about="http://purl.obolibrary.org/obo/GAZ_00253969">
        <obo:RO_0001025 rdf:resource="http://purl.obolibrary.org/obo/GAZ_00253968"/>
        <obo:IAO_0000115>A protected area. Established 2000.</obo:IAO_0000115>
        <oboInOwl:hasOBONamespace>GAZ</oboInOwl:hasOBONamespace>
        <oboInOwl:id>GAZ:00253969</oboInOwl:id>
        <rdfs:label>Tab Wildlife Management Area</rdfs:label>
    </owl:NamedIndividual>
    


    <!-- http://purl.obolibrary.org/obo/GAZ_00253970 -->

    <owl:NamedIndividual rdf:about="http://purl.obolibrary.org/obo/GAZ_00253970">
        <obo:RO_0001025 rdf:resource="http://purl.obolibrary.org/obo/GAZ_00253967"/>
        <obo:IAO_0000115>An island.</obo:IAO_0000115>
        <oboInOwl:hasOBONamespace>GAZ</oboInOwl:hasOBONamespace>
        <oboInOwl:id>GAZ:00253970</oboInOwl:id>
        <rdfs:label>Mazzaz Island</rdfs:label>
    </owl:NamedIndividual>
    


    <!-- http://purl.obolibrary.org/obo/GAZ_00253971 -->

    <owl:NamedIndividual rdf:about="http://purl.obolibrary.org/obo/GAZ_00253971">
        <obo:RO_0001025 rdf:resource="http://purl.obolibrary.org/obo/GAZ_00253967"/>
        <obo:IAO_0000115>An island.</obo:IAO_0000115>
        <oboInOwl:hasOBONamespace>GAZ</oboInOwl:hasOBONamespace>
        <oboInOwl:id>GAZ:00253971</oboInOwl:id>
        <rdfs:label>Paeowai Island</rdfs:label>
    </owl:NamedIndividual>
    


    <!-- http://purl.obolibrary.org/obo/GAZ_00253972 -->

    <owl:NamedIndividual rdf:about="http://purl.obolibrary.org/obo/GAZ_00253972">
        <obo:RO_0001025 rdf:resource="http://purl.obolibrary.org/obo/GAZ_00253968"/>
        <obo:IAO_0000115>A protected area. Located near Riwo Village, Madang Lagoon, Madang, Established 2002.</obo:IAO_0000115>
        <oboInOwl:hasOBONamespace>GAZ</oboInOwl:hasOBONamespace>
        <oboInOwl:id>GAZ:00253972</oboInOwl:id>
        <rdfs:label>Tabad Island Wildlife Management Area</rdfs:label>
    </owl:NamedIndividual>
    


    <!-- http://purl.obolibrary.org/obo/GAZ_00253973 -->

    <owl:NamedIndividual rdf:about="http://purl.obolibrary.org/obo/GAZ_00253973">
        <obo:RO_0001025 rdf:resource="http://purl.obolibrary.org/obo/GAZ_00253972"/>
        <obo:IAO_0000115>An island.</obo:IAO_0000115>
        <oboInOwl:hasOBONamespace>GAZ</oboInOwl:hasOBONamespace>
        <oboInOwl:id>GAZ:00253973</oboInOwl:id>
        <rdfs:label>Tabad Island</rdfs:label>
    </owl:NamedIndividual>
    


    <!-- http://purl.obolibrary.org/obo/GAZ_00253974 -->

    <owl:NamedIndividual rdf:about="http://purl.obolibrary.org/obo/GAZ_00253974">
        <obo:RO_0001025 rdf:resource="http://purl.obolibrary.org/obo/GAZ_00007255"/>
        <obo:IAO_0000115>An island.</obo:IAO_0000115>
        <oboInOwl:hasOBONamespace>GAZ</oboInOwl:hasOBONamespace>
        <oboInOwl:id>GAZ:00253974</oboInOwl:id>
        <rdfs:label>Lasanga Island</rdfs:label>
    </owl:NamedIndividual>
    


    <!-- http://purl.obolibrary.org/obo/GAZ_00253975 -->

    <owl:NamedIndividual rdf:about="http://purl.obolibrary.org/obo/GAZ_00253975">
        <obo:RO_0001025 rdf:resource="http://purl.obolibrary.org/obo/GAZ_00253974"/>
        <obo:IAO_0000115>A protected area. Established 1996.</obo:IAO_0000115>
        <oboInOwl:hasOBONamespace>GAZ</oboInOwl:hasOBONamespace>
        <oboInOwl:id>GAZ:00253975</oboInOwl:id>
        <rdfs:label>Kamiali Wildlife Management Area</rdfs:label>
    </owl:NamedIndividual>
    


    <!-- http://purl.obolibrary.org/obo/GAZ_00253976 -->

    <owl:NamedIndividual rdf:about="http://purl.obolibrary.org/obo/GAZ_00253976">
        <obo:RO_0001025 rdf:resource="http://purl.obolibrary.org/obo/GAZ_00012657"/>
        <obo:IAO_0000115>A protected area. Located 48 km from Port Moresby. Established 1963.</obo:IAO_0000115>
        <oboInOwl:hasOBONamespace>GAZ</oboInOwl:hasOBONamespace>
        <oboInOwl:id>GAZ:00253976</oboInOwl:id>
        <rdfs:label>Varirata National Park</rdfs:label>
    </owl:NamedIndividual>
    


    <!-- http://purl.obolibrary.org/obo/GAZ_00253977 -->

    <owl:NamedIndividual rdf:about="http://purl.obolibrary.org/obo/GAZ_00253977">
        <obo:RO_0001025 rdf:resource="http://purl.obolibrary.org/obo/GAZ_00118294"/>
        <obo:IAO_0000115>A protected area.</obo:IAO_0000115>
        <oboInOwl:hasOBONamespace>GAZ</oboInOwl:hasOBONamespace>
        <oboInOwl:id>GAZ:00253977</oboInOwl:id>
        <rdfs:label>Pocklington Reef Marine Reserve</rdfs:label>
    </owl:NamedIndividual>
    


    <!-- http://purl.obolibrary.org/obo/GAZ_00253978 -->

    <owl:NamedIndividual rdf:about="http://purl.obolibrary.org/obo/GAZ_00253978">
        <obo:RO_0001025 rdf:resource="http://purl.obolibrary.org/obo/GAZ_00012665"/>
        <obo:IAO_0000115>A protected area. Established 1975.</obo:IAO_0000115>
        <oboInOwl:hasOBONamespace>GAZ</oboInOwl:hasOBONamespace>
        <oboInOwl:id>GAZ:00253978</oboInOwl:id>
        <rdfs:label>Tonda Wildlife Management Area</rdfs:label>
    </owl:NamedIndividual>
    


    <!-- http://purl.obolibrary.org/obo/GAZ_00253979 -->

    <owl:NamedIndividual rdf:about="http://purl.obolibrary.org/obo/GAZ_00253979">
        <obo:RO_0001025 rdf:resource="http://purl.obolibrary.org/obo/GAZ_00005198"/>
        <obo:IAO_0000115>A protected area. Established 2001.</obo:IAO_0000115>
        <oboInOwl:hasOBONamespace>GAZ</oboInOwl:hasOBONamespace>
        <oboInOwl:id>GAZ:00253979</oboInOwl:id>
        <rdfs:label>Laugum Wildlife Management Area</rdfs:label>
    </owl:NamedIndividual>
    


    <!-- http://purl.obolibrary.org/obo/GAZ_00253980 -->

    <owl:NamedIndividual rdf:about="http://purl.obolibrary.org/obo/GAZ_00253980">
        <obo:RO_0001025 rdf:resource="http://purl.obolibrary.org/obo/GAZ_00012664"/>
        <obo:IAO_0000115>A protected area. Established 1992.</obo:IAO_0000115>
        <oboInOwl:hasOBONamespace>GAZ</oboInOwl:hasOBONamespace>
        <oboInOwl:id>GAZ:00253980</oboInOwl:id>
        <rdfs:label>Lake Kutubu Wildlife Management Area</rdfs:label>
    </owl:NamedIndividual>
    


    <!-- http://purl.obolibrary.org/obo/GAZ_00253981 -->

    <owl:NamedIndividual rdf:about="http://purl.obolibrary.org/obo/GAZ_00253981">
        <obo:RO_0001025 rdf:resource="http://purl.obolibrary.org/obo/GAZ_00012659"/>
        <obo:IAO_0000115>A protected area. Established 1996.</obo:IAO_0000115>
        <oboInOwl:hasOBONamespace>GAZ</oboInOwl:hasOBONamespace>
        <oboInOwl:id>GAZ:00253981</oboInOwl:id>
        <rdfs:label>Kikori Integrated Conservation and Development Project Area</rdfs:label>
    </owl:NamedIndividual>
    


    <!-- http://purl.obolibrary.org/obo/GAZ_00253982 -->

    <owl:NamedIndividual rdf:about="http://purl.obolibrary.org/obo/GAZ_00253982">
        <obo:RO_0001025 rdf:resource="http://purl.obolibrary.org/obo/GAZ_00253805"/>
        <obo:IAO_0000115>A protected area. Established 1981.</obo:IAO_0000115>
        <oboInOwl:hasOBONamespace>GAZ</oboInOwl:hasOBONamespace>
        <oboInOwl:id>GAZ:00253982</oboInOwl:id>
        <rdfs:label>Horseshoe Reef Marine Park</rdfs:label>
    </owl:NamedIndividual>
    


    <!-- http://purl.obolibrary.org/obo/GAZ_00253983 -->

    <owl:NamedIndividual rdf:about="http://purl.obolibrary.org/obo/GAZ_00253983">
        <obo:RO_0001025 rdf:resource="http://purl.obolibrary.org/obo/GAZ_00012664"/>
        <obo:IAO_0000115>A protected area.</obo:IAO_0000115>
        <oboInOwl:hasOBONamespace>GAZ</oboInOwl:hasOBONamespace>
        <oboInOwl:id>GAZ:00253983</oboInOwl:id>
        <rdfs:label>Mount Bosavi National Park</rdfs:label>
    </owl:NamedIndividual>
    


    <!-- http://purl.obolibrary.org/obo/GAZ_00253984 -->

    <owl:NamedIndividual rdf:about="http://purl.obolibrary.org/obo/GAZ_00253984">
        <obo:RO_0001025 rdf:resource="http://purl.obolibrary.org/obo/GAZ_00012657"/>
        <obo:IAO_0000115>A protected area. Established 1979.</obo:IAO_0000115>
        <oboInOwl:hasOBONamespace>GAZ</oboInOwl:hasOBONamespace>
        <oboInOwl:id>GAZ:00253984</oboInOwl:id>
        <rdfs:label>Namanatabu Historic Reserve</rdfs:label>
    </owl:NamedIndividual>
    


    <!-- http://purl.obolibrary.org/obo/GAZ_00253985 -->

    <owl:NamedIndividual rdf:about="http://purl.obolibrary.org/obo/GAZ_00253985">
        <obo:RO_0001025 rdf:resource="http://purl.obolibrary.org/obo/GAZ_00005198"/>
        <obo:IAO_0000115>A protected area.</obo:IAO_0000115>
        <oboInOwl:hasOBONamespace>GAZ</oboInOwl:hasOBONamespace>
        <oboInOwl:id>GAZ:00253985</oboInOwl:id>
        <rdfs:label>Adelbert Mountains Conservation Project Area</rdfs:label>
    </owl:NamedIndividual>
    


    <!-- http://purl.obolibrary.org/obo/GAZ_00253986 -->

    <owl:NamedIndividual rdf:about="http://purl.obolibrary.org/obo/GAZ_00253986">
        <obo:RO_0001025 rdf:resource="http://purl.obolibrary.org/obo/GAZ_00005193"/>
        <obo:IAO_0000115>A group of islands located 18 km south-southeast from Baluan and 32 km northeast from the reefs of the Alim Islands. The group consists of two islets located at either end of a 1.9 km long reef; a small submerged reef lies 1.2 km to the southwest.</obo:IAO_0000115>
        <oboInOwl:hasOBONamespace>GAZ</oboInOwl:hasOBONamespace>
        <oboInOwl:id>GAZ:00253986</oboInOwl:id>
        <rdfs:label>Papialou Islands</rdfs:label>
    </owl:NamedIndividual>
    


    <!-- http://purl.obolibrary.org/obo/GAZ_00253988 -->

    <owl:NamedIndividual rdf:about="http://purl.obolibrary.org/obo/GAZ_00253988">
        <obo:RO_0001025 rdf:resource="http://purl.obolibrary.org/obo/GAZ_00118291"/>
        <obo:IAO_0000115>A samll reef formation is located at the southeastern end of the Goschen Strait. The reef is located 8 km from Cape Ventenat, the southeastern tip of Normanby Island.</obo:IAO_0000115>
        <oboInOwl:hasOBONamespace>GAZ</oboInOwl:hasOBONamespace>
        <oboInOwl:id>GAZ:00253988</oboInOwl:id>
        <rdfs:label>Gallows Reef</rdfs:label>
    </owl:NamedIndividual>
    


    <!-- http://purl.obolibrary.org/obo/GAZ_00253989 -->

    <owl:NamedIndividual rdf:about="http://purl.obolibrary.org/obo/GAZ_00253989">
        <obo:RO_0001025 rdf:resource="http://purl.obolibrary.org/obo/GAZ_00253988"/>
        <obo:IAO_0000115>A sand cay located on Gallows Reef.</obo:IAO_0000115>
        <oboInOwl:hasOBONamespace>GAZ</oboInOwl:hasOBONamespace>
        <oboInOwl:id>GAZ:00253989</oboInOwl:id>
        <rdfs:label>Jack Island</rdfs:label>
    </owl:NamedIndividual>
    


    <!-- http://purl.obolibrary.org/obo/GAZ_00253990 -->

    <owl:NamedIndividual rdf:about="http://purl.obolibrary.org/obo/GAZ_00253990">
        <obo:RO_0001025 rdf:resource="http://purl.obolibrary.org/obo/GAZ_00253988"/>
        <obo:IAO_0000115>A sand cay located on Gallows Reef.</obo:IAO_0000115>
        <oboInOwl:hasOBONamespace>GAZ</oboInOwl:hasOBONamespace>
        <oboInOwl:id>GAZ:00253990</oboInOwl:id>
        <rdfs:label>Ketch Island</rdfs:label>
    </owl:NamedIndividual>
    


    <!-- http://purl.obolibrary.org/obo/GAZ_00253991 -->

    <owl:NamedIndividual rdf:about="http://purl.obolibrary.org/obo/GAZ_00253991">
        <obo:RO_0001025 rdf:resource="http://purl.obolibrary.org/obo/GAZ_00053904"/>
        <obo:IAO_0000115>One of the Mundua Islands.</obo:IAO_0000115>
        <oboInOwl:hasOBONamespace>GAZ</oboInOwl:hasOBONamespace>
        <oboInOwl:id>GAZ:00253991</oboInOwl:id>
        <rdfs:label>Vambu Island</rdfs:label>
    </owl:NamedIndividual>
    


    <!-- http://purl.obolibrary.org/obo/GAZ_00253992 -->

    <owl:NamedIndividual rdf:about="http://purl.obolibrary.org/obo/GAZ_00253992">
        <obo:RO_0001025 rdf:resource="http://purl.obolibrary.org/obo/GAZ_00053904"/>
        <obo:IAO_0000115>One of the Mundua Islands.</obo:IAO_0000115>
        <oboInOwl:hasOBONamespace>GAZ</oboInOwl:hasOBONamespace>
        <oboInOwl:id>GAZ:00253992</oboInOwl:id>
        <rdfs:label>Undaga Island</rdfs:label>
    </owl:NamedIndividual>
    


    <!-- http://purl.obolibrary.org/obo/GAZ_00253993 -->

    <owl:NamedIndividual rdf:about="http://purl.obolibrary.org/obo/GAZ_00253993">
        <obo:RO_0001025 rdf:resource="http://purl.obolibrary.org/obo/GAZ_00007179"/>
        <obo:IAO_0000115>Asubmerged, atoll-like reef of the Admiralty Islands group of the northwestern Bismarck Sea. The reef lies 5 km outside the extensive barrier reefs that surround the southwestern coast of Manus Island; the southern coast of Manus itself is located 14 km to the north. Larsen Reef has an irregular outline, approximately circular in shape, with a diameter of up to 10 km. A deep central lagoon is partially enclosed by a series of submerged, linear reefs that are separated by wide passages.</obo:IAO_0000115>
        <oboInOwl:hasOBONamespace>GAZ</oboInOwl:hasOBONamespace>
        <oboInOwl:id>GAZ:00253993</oboInOwl:id>
        <rdfs:label>Larsen Reef</rdfs:label>
    </owl:NamedIndividual>
    


    <!-- http://purl.obolibrary.org/obo/GAZ_00253998 -->

    <owl:NamedIndividual rdf:about="http://purl.obolibrary.org/obo/GAZ_00253998">
        <obo:RO_0001025 rdf:resource="http://purl.obolibrary.org/obo/GAZ_00146838"/>
        <obo:IAO_0000115>An arcuate reef structure located within the central regions of New Britain&apos;s Kimbe Bay.</obo:IAO_0000115>
        <oboInOwl:hasOBONamespace>GAZ</oboInOwl:hasOBONamespace>
        <oboInOwl:id>GAZ:00253998</oboInOwl:id>
        <rdfs:label>Oto Reef</rdfs:label>
    </owl:NamedIndividual>
    


    <!-- http://purl.obolibrary.org/obo/GAZ_00253999 -->

    <owl:NamedIndividual rdf:about="http://purl.obolibrary.org/obo/GAZ_00253999">
        <obo:RO_0001025 rdf:resource="http://purl.obolibrary.org/obo/GAZ_00016847"/>
        <obo:IAO_0000115>A western outlier of the Vitu Islands group. The reef lies 35 km northwest from the small island of Narage in the Vitu Islands proper and some 63 km from the Whirlwind Reefs.</obo:IAO_0000115>
        <oboInOwl:hasOBONamespace>GAZ</oboInOwl:hasOBONamespace>
        <oboInOwl:id>GAZ:00253999</oboInOwl:id>
        <rdfs:label>Ottilien Reef</rdfs:label>
    </owl:NamedIndividual>
    


    <!-- http://purl.obolibrary.org/obo/GAZ_00254000 -->

    <owl:NamedIndividual rdf:about="http://purl.obolibrary.org/obo/GAZ_00254000">
        <obo:RO_0001025 rdf:resource="http://purl.obolibrary.org/obo/GAZ_00007179"/>
        <obo:IAO_0000115>A small group of islands that make up part of the large Admiralty Islands group of northwestern Papua New Guinea. They are located 17 km west from Rambutyo and 34 km southeast from Manus; the Fedarb Islands lie 8.5 km to the southwest.</obo:IAO_0000115>
        <oboInOwl:hasOBONamespace>GAZ</oboInOwl:hasOBONamespace>
        <oboInOwl:id>GAZ:00254000</oboInOwl:id>
        <rdfs:label>San Miguel Islands</rdfs:label>
    </owl:NamedIndividual>
    


    <!-- http://purl.obolibrary.org/obo/GAZ_00254001 -->

    <owl:NamedIndividual rdf:about="http://purl.obolibrary.org/obo/GAZ_00254001">
        <obo:RO_0001025 rdf:resource="http://purl.obolibrary.org/obo/GAZ_00254000"/>
        <obo:IAO_0000115>An island consisting of an outer reef ring, sunken in the east, south and west, and two islets, one on the northeastern reef rim and one within the interior lagoon.</obo:IAO_0000115>
        <oboInOwl:hasOBONamespace>GAZ</oboInOwl:hasOBONamespace>
        <oboInOwl:id>GAZ:00254001</oboInOwl:id>
        <rdfs:label>Anobat Island</rdfs:label>
    </owl:NamedIndividual>
    


    <!-- http://purl.obolibrary.org/obo/GAZ_00254002 -->

    <owl:NamedIndividual rdf:about="http://purl.obolibrary.org/obo/GAZ_00254002">
        <obo:RO_0001025 rdf:resource="http://purl.obolibrary.org/obo/GAZ_00254000"/>
        <obo:IAO_0000115>An atoll? with several islands that enclose an interior lagoon.</obo:IAO_0000115>
        <oboInOwl:hasOBONamespace>GAZ</oboInOwl:hasOBONamespace>
        <oboInOwl:id>GAZ:00254002</oboInOwl:id>
        <rdfs:label>Loraine Island</rdfs:label>
    </owl:NamedIndividual>
    


    <!-- http://purl.obolibrary.org/obo/GAZ_00254003 -->

    <owl:NamedIndividual rdf:about="http://purl.obolibrary.org/obo/GAZ_00254003">
        <obo:RO_0001025 rdf:resource="http://purl.obolibrary.org/obo/GAZ_00007182"/>
        <obo:IAO_0000115>An island that lies 1.1 km across the narrow China Strait from the southwestern tip of New Guinea. It is one of several large and numerous smaller islands that extend to the southeast between the mainland and the islands of the Engineer Group. Its significant neighbours include the island of Sideia (located immediately off its eastern extremity) and Samarai (located to the southwest across the East Channel).</obo:IAO_0000115>
        <oboInOwl:hasOBONamespace>GAZ</oboInOwl:hasOBONamespace>
        <oboInOwl:id>GAZ:00254003</oboInOwl:id>
        <rdfs:label>Sariba</rdfs:label>
    </owl:NamedIndividual>
    


    <!-- http://purl.obolibrary.org/obo/GAZ_00254009 -->

    <owl:NamedIndividual rdf:about="http://purl.obolibrary.org/obo/GAZ_00254009">
        <obo:RO_0001025 rdf:resource="http://purl.obolibrary.org/obo/GAZ_00016822"/>
        <obo:IAO_0000115>A minor reef formation located at the western edge of the Admiralty Islands group.</obo:IAO_0000115>
        <oboInOwl:hasOBONamespace>GAZ</oboInOwl:hasOBONamespace>
        <oboInOwl:id>GAZ:00254009</oboInOwl:id>
        <rdfs:label>Western Reef</rdfs:label>
    </owl:NamedIndividual>
    


    <!-- http://purl.obolibrary.org/obo/GAZ_00254010 -->

    <owl:NamedIndividual rdf:about="http://purl.obolibrary.org/obo/GAZ_00254010">
        <obo:RO_0001025 rdf:resource="http://purl.obolibrary.org/obo/GAZ_00005191"/>
        <obo:IAO_0000115>Town island just N of New Britain.</obo:IAO_0000115>
        <oboInOwl:hasOBONamespace>GAZ</oboInOwl:hasOBONamespace>
        <oboInOwl:id>GAZ:00254010</oboInOwl:id>
        <rdfs:label>Wulai Islands</rdfs:label>
    </owl:NamedIndividual>
    


    <!-- 
    ///////////////////////////////////////////////////////////////////////////////////////
    //
    // Annotations
    //
    ///////////////////////////////////////////////////////////////////////////////////////
     -->

    <rdf:Description rdf:about="http://purl.obolibrary.org/obo/GAZ_00005195">
        <rdfs:label>Kieta</rdfs:label>
        <oboInOwl:hasOBONamespace>GAZ</oboInOwl:hasOBONamespace>
        <oboInOwl:id>GAZ:00005195</oboInOwl:id>
    </rdf:Description>
    <rdf:Description rdf:about="http://purl.obolibrary.org/obo/GAZ_00005196">
        <oboInOwl:hasOBONamespace>GAZ</oboInOwl:hasOBONamespace>
        <rdfs:label>populated place, Papua New Guinea</rdfs:label>
        <oboInOwl:id>GAZ:00005196</oboInOwl:id>
    </rdf:Description>
    <rdf:Description rdf:about="http://purl.obolibrary.org/obo/GAZ_00005197">
        <oboInOwl:hasOBONamespace>GAZ</oboInOwl:hasOBONamespace>
        <rdfs:label>Buin</rdfs:label>
        <oboInOwl:id>GAZ:00005197</oboInOwl:id>
    </rdf:Description>
    <rdf:Description rdf:about="http://purl.obolibrary.org/obo/GAZ_00005199">
        <oboInOwl:id>GAZ:00005199</oboInOwl:id>
        <rdfs:label>Baiteta</rdfs:label>
        <oboInOwl:hasOBONamespace>GAZ</oboInOwl:hasOBONamespace>
    </rdf:Description>
    <rdf:Description rdf:about="http://purl.obolibrary.org/obo/GAZ_00005205">
        <oboInOwl:id>GAZ:00005205</oboInOwl:id>
        <oboInOwl:hasOBONamespace>GAZ</oboInOwl:hasOBONamespace>
        <rdfs:label>Amron Village</rdfs:label>
    </rdf:Description>
    <rdf:Description rdf:about="http://purl.obolibrary.org/obo/GAZ_00005217">
        <oboInOwl:id>GAZ:00005217</oboInOwl:id>
        <obo:IAO_0000115>A populated place. A township of East New Britain province, Papua New Guinea. The town was the provincial capital and most important settlement in the province until it was destroyed in 1994 by falling ash of a volcanic eruption.</obo:IAO_0000115>
        <oboInOwl:hasOBONamespace>GAZ</oboInOwl:hasOBONamespace>
        <rdfs:label>Rabaul</rdfs:label>
    </rdf:Description>
    <rdf:Description rdf:about="http://purl.obolibrary.org/obo/GAZ_00005263">
        <rdfs:label>Port Moresby</rdfs:label>
        <oboInOwl:id>GAZ:00005263</oboInOwl:id>
        <oboInOwl:hasOBONamespace>GAZ</oboInOwl:hasOBONamespace>
        <obo:IAO_0000115>The capital and largest city of Papua New Guinea (PNG). The city is located on the shores of the Gulf of Papua, on the southeastern coast of the island of New Guinea.</obo:IAO_0000115>
    </rdf:Description>
    <rdf:Description rdf:about="http://purl.obolibrary.org/obo/GAZ_00005267">
        <oboInOwl:hasOBONamespace>GAZ</oboInOwl:hasOBONamespace>
        <obo:IAO_0000115>The capital of the East Sepik province of Papua New Guinea. It is located on the northern coast of the island of New Guinea.</obo:IAO_0000115>
        <rdfs:label>Wewak</rdfs:label>
        <oboInOwl:id>GAZ:00005267</oboInOwl:id>
    </rdf:Description>
    <rdf:Description rdf:about="http://purl.obolibrary.org/obo/GAZ_00007257">
        <oboInOwl:hasOBONamespace>GAZ</oboInOwl:hasOBONamespace>
        <rdfs:label>Finschhafen</rdfs:label>
        <oboInOwl:id>GAZ:00007257</oboInOwl:id>
    </rdf:Description>
    <rdf:Description rdf:about="http://purl.obolibrary.org/obo/GAZ_00010065">
        <oboInOwl:id>GAZ:00010065</oboInOwl:id>
        <oboInOwl:hasOBONamespace>GAZ</oboInOwl:hasOBONamespace>
        <rdfs:label>Goroka</rdfs:label>
    </rdf:Description>
    <rdf:Description rdf:about="http://purl.obolibrary.org/obo/GAZ_00016819">
        <rdfs:label>Manus Island</rdfs:label>
        <oboInOwl:hasOBONamespace>GAZ</oboInOwl:hasOBONamespace>
        <obo:IAO_0000115>A volcanic island that is part of Manus Province in northern Papua New Guinea and is the largest island of the Admiralty Islands.</obo:IAO_0000115>
        <oboInOwl:id>GAZ:00016819</oboInOwl:id>
    </rdf:Description>
    <rdf:Description rdf:about="http://purl.obolibrary.org/obo/GAZ_00117917">
        <oboInOwl:id>GAZ:00117917</oboInOwl:id>
        <oboInOwl:hasOBONamespace>GAZ</oboInOwl:hasOBONamespace>
        <rdfs:label>Region (Papua New Guinea)</rdfs:label>
    </rdf:Description>
    <rdf:Description rdf:about="http://purl.obolibrary.org/obo/GAZ_00117918">
        <obo:IAO_0000115>One of four regions of Papua New Guinea.</obo:IAO_0000115>
        <oboInOwl:id>GAZ:00117918</oboInOwl:id>
        <oboInOwl:hasOBONamespace>GAZ</oboInOwl:hasOBONamespace>
        <rdfs:label>Highlands Region</rdfs:label>
    </rdf:Description>
    <rdf:Description rdf:about="http://purl.obolibrary.org/obo/GAZ_00117919">
        <obo:IAO_0000115>One of four regions of Papua New Guinea.</obo:IAO_0000115>
        <oboInOwl:id>GAZ:00117919</oboInOwl:id>
        <oboInOwl:hasOBONamespace>GAZ</oboInOwl:hasOBONamespace>
        <rdfs:label>Momase Region</rdfs:label>
    </rdf:Description>
    <rdf:Description rdf:about="http://purl.obolibrary.org/obo/GAZ_00117920">
        <obo:IAO_0000115>One of four regions of Papua New Guinea.</obo:IAO_0000115>
        <oboInOwl:id>GAZ:00117920</oboInOwl:id>
        <rdfs:label>Islands Region</rdfs:label>
        <oboInOwl:hasOBONamespace>GAZ</oboInOwl:hasOBONamespace>
    </rdf:Description>
    <rdf:Description rdf:about="http://purl.obolibrary.org/obo/GAZ_00117921">
        <oboInOwl:id>GAZ:00117921</oboInOwl:id>
        <rdfs:label>Papua Region</rdfs:label>
        <oboInOwl:hasOBONamespace>GAZ</oboInOwl:hasOBONamespace>
        <obo:IAO_0000115>One of four regions of Papua New Guinea.</obo:IAO_0000115>
    </rdf:Description>
    <rdf:Description rdf:about="http://purl.obolibrary.org/obo/GAZ_00253640">
        <oboInOwl:hasOBONamespace>GAZ</oboInOwl:hasOBONamespace>
        <rdfs:label>Nakanai Mountains</rdfs:label>
        <obo:IAO_0000115>A mountain range.</obo:IAO_0000115>
        <oboInOwl:id>GAZ:00253640</oboInOwl:id>
    </rdf:Description>
</rdf:RDF>



<!-- Generated by the OWL API (version 4.5.6) https://github.com/owlcs/owlapi -->

