<?xml version="1.0"?>
<rdf:RDF xmlns="http://purl.obolibrary.org/obo/gaz/subsets/countries/Republic_of_Cyprus.owl#"
     xml:base="http://purl.obolibrary.org/obo/gaz/subsets/countries/Republic_of_Cyprus.owl"
     xmlns:obo="http://purl.obolibrary.org/obo/"
     xmlns:owl="http://www.w3.org/2002/07/owl#"
     xmlns:rdf="http://www.w3.org/1999/02/22-rdf-syntax-ns#"
     xmlns:xml="http://www.w3.org/XML/1998/namespace"
     xmlns:xsd="http://www.w3.org/2001/XMLSchema#"
     xmlns:rdfs="http://www.w3.org/2000/01/rdf-schema#"
     xmlns:oboInOwl="http://www.geneontology.org/formats/oboInOwl#">
    <owl:Ontology rdf:about="http://purl.obolibrary.org/obo/gaz/subsets/countries/Republic_of_Cyprus.owl">
        <owl:imports rdf:resource="http://purl.obolibrary.org/obo/gaz/imports/envo_import.owl"/>
        <owl:imports rdf:resource="http://purl.obolibrary.org/obo/gaz/imports/ro_import.owl"/>
    </owl:Ontology>
    


    <!-- 
    ///////////////////////////////////////////////////////////////////////////////////////
    //
    // Annotation properties
    //
    ///////////////////////////////////////////////////////////////////////////////////////
     -->

    


    <!-- http://purl.obolibrary.org/obo/IAO_0000115 -->

    <owl:AnnotationProperty rdf:about="http://purl.obolibrary.org/obo/IAO_0000115"/>
    


    <!-- http://www.geneontology.org/formats/oboInOwl#hasOBONamespace -->

    <owl:AnnotationProperty rdf:about="http://www.geneontology.org/formats/oboInOwl#hasOBONamespace"/>
    


    <!-- http://www.geneontology.org/formats/oboInOwl#id -->

    <owl:AnnotationProperty rdf:about="http://www.geneontology.org/formats/oboInOwl#id"/>
    


    <!-- 
    ///////////////////////////////////////////////////////////////////////////////////////
    //
    // Object Properties
    //
    ///////////////////////////////////////////////////////////////////////////////////////
     -->

    


    <!-- http://purl.obolibrary.org/obo/RO_0001025 -->

    <owl:ObjectProperty rdf:about="http://purl.obolibrary.org/obo/RO_0001025"/>
    


    <!-- 
    ///////////////////////////////////////////////////////////////////////////////////////
    //
    // Classes
    //
    ///////////////////////////////////////////////////////////////////////////////////////
     -->

    


    <!-- http://purl.obolibrary.org/obo/ENVO_00000856 -->

    <owl:Class rdf:about="http://purl.obolibrary.org/obo/ENVO_00000856"/>
    


    <!-- http://purl.obolibrary.org/obo/GAZ_00358442 -->

    <owl:Class rdf:about="http://purl.obolibrary.org/obo/GAZ_00358442">
        <rdfs:subClassOf rdf:resource="http://purl.obolibrary.org/obo/GAZ_02000434"/>
        <obo:IAO_0000115>One of the six districts of Cyprus. Controlled by the Turkish Republic of Northern Cyprus.</obo:IAO_0000115>
        <oboInOwl:hasOBONamespace>GAZ</oboInOwl:hasOBONamespace>
        <oboInOwl:id>GAZ:00358442</oboInOwl:id>
        <rdfs:label>Kyrenia District</rdfs:label>
    </owl:Class>
    


    <!-- http://purl.obolibrary.org/obo/GAZ_02000434 -->

    <owl:Class rdf:about="http://purl.obolibrary.org/obo/GAZ_02000434"/>
    


    <!-- http://purl.obolibrary.org/obo/GAZ_02000435 -->

    <owl:Class rdf:about="http://purl.obolibrary.org/obo/GAZ_02000435">
        <rdfs:subClassOf rdf:resource="http://purl.obolibrary.org/obo/GAZ_02000434"/>
    </owl:Class>
    


    <!-- http://purl.obolibrary.org/obo/GAZ_02000436 -->

    <owl:Class rdf:about="http://purl.obolibrary.org/obo/GAZ_02000436">
        <rdfs:subClassOf rdf:resource="http://purl.obolibrary.org/obo/GAZ_02000434"/>
    </owl:Class>
    


    <!-- http://purl.obolibrary.org/obo/GAZ_02000437 -->

    <owl:Class rdf:about="http://purl.obolibrary.org/obo/GAZ_02000437">
        <rdfs:subClassOf rdf:resource="http://purl.obolibrary.org/obo/GAZ_02000434"/>
    </owl:Class>
    


    <!-- http://purl.obolibrary.org/obo/GAZ_02000439 -->

    <owl:Class rdf:about="http://purl.obolibrary.org/obo/GAZ_02000439">
        <rdfs:subClassOf rdf:resource="http://purl.obolibrary.org/obo/GAZ_02000434"/>
    </owl:Class>
    


    <!-- http://purl.obolibrary.org/obo/GAZ_02000440 -->

    <owl:Class rdf:about="http://purl.obolibrary.org/obo/GAZ_02000440">
        <rdfs:subClassOf rdf:resource="http://purl.obolibrary.org/obo/GAZ_02000434"/>
    </owl:Class>
    


    <!-- 
    ///////////////////////////////////////////////////////////////////////////////////////
    //
    // Individuals
    //
    ///////////////////////////////////////////////////////////////////////////////////////
     -->

    


    <!-- http://purl.obolibrary.org/obo/GAZ_00004007 -->

    <owl:NamedIndividual rdf:about="http://purl.obolibrary.org/obo/GAZ_00004007">
        <obo:IAO_0000115>An internationally recognized state, has de jure sovereignty over 97% of the island of Cyprus and all surrounding waters.</obo:IAO_0000115>
        <oboInOwl:hasOBONamespace>GAZ</oboInOwl:hasOBONamespace>
        <oboInOwl:id>GAZ:00004007</oboInOwl:id>
        <rdfs:label>Republic of Cyprus</rdfs:label>
    </owl:NamedIndividual>
    


    <!-- http://purl.obolibrary.org/obo/GAZ_00028479 -->

    <owl:NamedIndividual rdf:about="http://purl.obolibrary.org/obo/GAZ_00028479">
        <obo:RO_0001025 rdf:resource="http://purl.obolibrary.org/obo/GAZ_02000437"/>
        <oboInOwl:hasOBONamespace>GAZ</oboInOwl:hasOBONamespace>
        <oboInOwl:id>GAZ:00028479</oboInOwl:id>
        <rdfs:label>Municipality of Paphos</rdfs:label>
    </owl:NamedIndividual>
    


    <!-- http://purl.obolibrary.org/obo/GAZ_00028480 -->

    <owl:NamedIndividual rdf:about="http://purl.obolibrary.org/obo/GAZ_00028480">
        <obo:RO_0001025 rdf:resource="http://purl.obolibrary.org/obo/GAZ_02000437"/>
        <oboInOwl:hasOBONamespace>GAZ</oboInOwl:hasOBONamespace>
        <oboInOwl:id>GAZ:00028480</oboInOwl:id>
        <rdfs:label>Municipality of Yeroskipou</rdfs:label>
    </owl:NamedIndividual>
    


    <!-- http://purl.obolibrary.org/obo/GAZ_00028481 -->

    <owl:NamedIndividual rdf:about="http://purl.obolibrary.org/obo/GAZ_00028481">
        <obo:RO_0001025 rdf:resource="http://purl.obolibrary.org/obo/GAZ_02000437"/>
        <oboInOwl:hasOBONamespace>GAZ</oboInOwl:hasOBONamespace>
        <oboInOwl:id>GAZ:00028481</oboInOwl:id>
        <rdfs:label>Municipality of Polis Chrysochous</rdfs:label>
    </owl:NamedIndividual>
    


    <!-- http://purl.obolibrary.org/obo/GAZ_00028482 -->

    <owl:NamedIndividual rdf:about="http://purl.obolibrary.org/obo/GAZ_00028482">
        <obo:RO_0001025 rdf:resource="http://purl.obolibrary.org/obo/GAZ_02000437"/>
        <oboInOwl:hasOBONamespace>GAZ</oboInOwl:hasOBONamespace>
        <oboInOwl:id>GAZ:00028482</oboInOwl:id>
        <rdfs:label>Municipality of Peyia</rdfs:label>
    </owl:NamedIndividual>
    


    <!-- http://purl.obolibrary.org/obo/GAZ_00028488 -->

    <owl:NamedIndividual rdf:about="http://purl.obolibrary.org/obo/GAZ_00028488">
        <obo:RO_0001025 rdf:resource="http://purl.obolibrary.org/obo/GAZ_02000440"/>
        <oboInOwl:hasOBONamespace>GAZ</oboInOwl:hasOBONamespace>
        <oboInOwl:id>GAZ:00028488</oboInOwl:id>
        <rdfs:label>Municipality of Aradippou</rdfs:label>
    </owl:NamedIndividual>
    


    <!-- http://purl.obolibrary.org/obo/GAZ_00028489 -->

    <owl:NamedIndividual rdf:about="http://purl.obolibrary.org/obo/GAZ_00028489">
        <obo:RO_0001025 rdf:resource="http://purl.obolibrary.org/obo/GAZ_02000440"/>
        <oboInOwl:hasOBONamespace>GAZ</oboInOwl:hasOBONamespace>
        <oboInOwl:id>GAZ:00028489</oboInOwl:id>
        <rdfs:label>Municipality of Lefkara</rdfs:label>
    </owl:NamedIndividual>
    


    <!-- http://purl.obolibrary.org/obo/GAZ_00028491 -->

    <owl:NamedIndividual rdf:about="http://purl.obolibrary.org/obo/GAZ_00028491">
        <obo:RO_0001025 rdf:resource="http://purl.obolibrary.org/obo/GAZ_02000440"/>
        <oboInOwl:hasOBONamespace>GAZ</oboInOwl:hasOBONamespace>
        <oboInOwl:id>GAZ:00028491</oboInOwl:id>
        <rdfs:label>Municipality of Larnaca</rdfs:label>
    </owl:NamedIndividual>
    


    <!-- http://purl.obolibrary.org/obo/GAZ_00028492 -->

    <owl:NamedIndividual rdf:about="http://purl.obolibrary.org/obo/GAZ_00028492">
        <obo:RO_0001025 rdf:resource="http://purl.obolibrary.org/obo/GAZ_02000440"/>
        <oboInOwl:hasOBONamespace>GAZ</oboInOwl:hasOBONamespace>
        <oboInOwl:id>GAZ:00028492</oboInOwl:id>
        <rdfs:label>Municipality of Athienou</rdfs:label>
    </owl:NamedIndividual>
    


    <!-- http://purl.obolibrary.org/obo/GAZ_00028493 -->

    <owl:NamedIndividual rdf:about="http://purl.obolibrary.org/obo/GAZ_00028493">
        <obo:RO_0001025 rdf:resource="http://purl.obolibrary.org/obo/GAZ_02000439"/>
        <oboInOwl:hasOBONamespace>GAZ</oboInOwl:hasOBONamespace>
        <oboInOwl:id>GAZ:00028493</oboInOwl:id>
        <rdfs:label>Nicosia South</rdfs:label>
    </owl:NamedIndividual>
    


    <!-- http://purl.obolibrary.org/obo/GAZ_00028500 -->

    <owl:NamedIndividual rdf:about="http://purl.obolibrary.org/obo/GAZ_00028500">
        <obo:RO_0001025 rdf:resource="http://purl.obolibrary.org/obo/GAZ_00028493"/>
        <oboInOwl:hasOBONamespace>GAZ</oboInOwl:hasOBONamespace>
        <oboInOwl:id>GAZ:00028500</oboInOwl:id>
        <rdfs:label>Municipality of Idalion</rdfs:label>
    </owl:NamedIndividual>
    


    <!-- http://purl.obolibrary.org/obo/GAZ_00028501 -->

    <owl:NamedIndividual rdf:about="http://purl.obolibrary.org/obo/GAZ_00028501">
        <obo:RO_0001025 rdf:resource="http://purl.obolibrary.org/obo/GAZ_00028493"/>
        <oboInOwl:hasOBONamespace>GAZ</oboInOwl:hasOBONamespace>
        <oboInOwl:id>GAZ:00028501</oboInOwl:id>
        <rdfs:label>Municipality of Ayios Dhometios</rdfs:label>
    </owl:NamedIndividual>
    


    <!-- http://purl.obolibrary.org/obo/GAZ_00028503 -->

    <owl:NamedIndividual rdf:about="http://purl.obolibrary.org/obo/GAZ_00028503">
        <obo:RO_0001025 rdf:resource="http://purl.obolibrary.org/obo/GAZ_00028493"/>
        <oboInOwl:hasOBONamespace>GAZ</oboInOwl:hasOBONamespace>
        <oboInOwl:id>GAZ:00028503</oboInOwl:id>
        <rdfs:label>Municipality of Lakatamia</rdfs:label>
    </owl:NamedIndividual>
    


    <!-- http://purl.obolibrary.org/obo/GAZ_00028504 -->

    <owl:NamedIndividual rdf:about="http://purl.obolibrary.org/obo/GAZ_00028504">
        <obo:RO_0001025 rdf:resource="http://purl.obolibrary.org/obo/GAZ_00028493"/>
        <oboInOwl:hasOBONamespace>GAZ</oboInOwl:hasOBONamespace>
        <oboInOwl:id>GAZ:00028504</oboInOwl:id>
        <rdfs:label>Municipality of Karavas</rdfs:label>
    </owl:NamedIndividual>
    


    <!-- http://purl.obolibrary.org/obo/GAZ_00028505 -->

    <owl:NamedIndividual rdf:about="http://purl.obolibrary.org/obo/GAZ_00028505">
        <obo:RO_0001025 rdf:resource="http://purl.obolibrary.org/obo/GAZ_00028493"/>
        <oboInOwl:hasOBONamespace>GAZ</oboInOwl:hasOBONamespace>
        <oboInOwl:id>GAZ:00028505</oboInOwl:id>
        <rdfs:label>Municipality of Kythrea</rdfs:label>
    </owl:NamedIndividual>
    


    <!-- http://purl.obolibrary.org/obo/GAZ_00028506 -->

    <owl:NamedIndividual rdf:about="http://purl.obolibrary.org/obo/GAZ_00028506">
        <obo:RO_0001025 rdf:resource="http://purl.obolibrary.org/obo/GAZ_00028493"/>
        <oboInOwl:hasOBONamespace>GAZ</oboInOwl:hasOBONamespace>
        <oboInOwl:id>GAZ:00028506</oboInOwl:id>
        <rdfs:label>Municipality of Strovolos</rdfs:label>
    </owl:NamedIndividual>
    


    <!-- http://purl.obolibrary.org/obo/GAZ_00028507 -->

    <owl:NamedIndividual rdf:about="http://purl.obolibrary.org/obo/GAZ_00028507">
        <obo:RO_0001025 rdf:resource="http://purl.obolibrary.org/obo/GAZ_00028493"/>
        <oboInOwl:hasOBONamespace>GAZ</oboInOwl:hasOBONamespace>
        <oboInOwl:id>GAZ:00028507</oboInOwl:id>
        <rdfs:label>Municipality of Aglantzia</rdfs:label>
    </owl:NamedIndividual>
    


    <!-- http://purl.obolibrary.org/obo/GAZ_00028508 -->

    <owl:NamedIndividual rdf:about="http://purl.obolibrary.org/obo/GAZ_00028508">
        <obo:RO_0001025 rdf:resource="http://purl.obolibrary.org/obo/GAZ_00028493"/>
        <oboInOwl:hasOBONamespace>GAZ</oboInOwl:hasOBONamespace>
        <oboInOwl:id>GAZ:00028508</oboInOwl:id>
        <rdfs:label>Municipality of Engomi</rdfs:label>
    </owl:NamedIndividual>
    


    <!-- http://purl.obolibrary.org/obo/GAZ_00028509 -->

    <owl:NamedIndividual rdf:about="http://purl.obolibrary.org/obo/GAZ_00028509">
        <obo:RO_0001025 rdf:resource="http://purl.obolibrary.org/obo/GAZ_00028493"/>
        <oboInOwl:hasOBONamespace>GAZ</oboInOwl:hasOBONamespace>
        <oboInOwl:id>GAZ:00028509</oboInOwl:id>
        <rdfs:label>Municipality of Latsia</rdfs:label>
    </owl:NamedIndividual>
    


    <!-- http://purl.obolibrary.org/obo/GAZ_00028510 -->

    <owl:NamedIndividual rdf:about="http://purl.obolibrary.org/obo/GAZ_00028510">
        <obo:RO_0001025 rdf:resource="http://purl.obolibrary.org/obo/GAZ_00028493"/>
        <oboInOwl:hasOBONamespace>GAZ</oboInOwl:hasOBONamespace>
        <oboInOwl:id>GAZ:00028510</oboInOwl:id>
        <rdfs:label>Municipality of Lapithos</rdfs:label>
    </owl:NamedIndividual>
    


    <!-- http://purl.obolibrary.org/obo/GAZ_00028523 -->

    <owl:NamedIndividual rdf:about="http://purl.obolibrary.org/obo/GAZ_00028523">
        <obo:RO_0001025 rdf:resource="http://purl.obolibrary.org/obo/GAZ_02000436"/>
        <oboInOwl:hasOBONamespace>GAZ</oboInOwl:hasOBONamespace>
        <oboInOwl:id>GAZ:00028523</oboInOwl:id>
        <rdfs:label>Municipality of Paralimni</rdfs:label>
    </owl:NamedIndividual>
    


    <!-- http://purl.obolibrary.org/obo/GAZ_00028525 -->

    <owl:NamedIndividual rdf:about="http://purl.obolibrary.org/obo/GAZ_00028525">
        <obo:RO_0001025 rdf:resource="http://purl.obolibrary.org/obo/GAZ_02000436"/>
        <oboInOwl:hasOBONamespace>GAZ</oboInOwl:hasOBONamespace>
        <oboInOwl:id>GAZ:00028525</oboInOwl:id>
        <rdfs:label>Municipality of Ayia Napa</rdfs:label>
    </owl:NamedIndividual>
    


    <!-- http://purl.obolibrary.org/obo/GAZ_00028526 -->

    <owl:NamedIndividual rdf:about="http://purl.obolibrary.org/obo/GAZ_00028526">
        <obo:RO_0001025 rdf:resource="http://purl.obolibrary.org/obo/GAZ_02000436"/>
        <oboInOwl:hasOBONamespace>GAZ</oboInOwl:hasOBONamespace>
        <oboInOwl:id>GAZ:00028526</oboInOwl:id>
        <rdfs:label>Municipality of Dherynia</rdfs:label>
    </owl:NamedIndividual>
    


    <!-- http://purl.obolibrary.org/obo/GAZ_00028531 -->

    <owl:NamedIndividual rdf:about="http://purl.obolibrary.org/obo/GAZ_00028531">
        <obo:RO_0001025 rdf:resource="http://purl.obolibrary.org/obo/GAZ_02000435"/>
        <oboInOwl:hasOBONamespace>GAZ</oboInOwl:hasOBONamespace>
        <oboInOwl:id>GAZ:00028531</oboInOwl:id>
        <rdfs:label>Municipality of Ayios Athanasios</rdfs:label>
    </owl:NamedIndividual>
    


    <!-- http://purl.obolibrary.org/obo/GAZ_00028532 -->

    <owl:NamedIndividual rdf:about="http://purl.obolibrary.org/obo/GAZ_00028532">
        <obo:RO_0001025 rdf:resource="http://purl.obolibrary.org/obo/GAZ_02000435"/>
        <oboInOwl:hasOBONamespace>GAZ</oboInOwl:hasOBONamespace>
        <oboInOwl:id>GAZ:00028532</oboInOwl:id>
        <rdfs:label>Municipality of Mesa Yitonia</rdfs:label>
    </owl:NamedIndividual>
    


    <!-- http://purl.obolibrary.org/obo/GAZ_00028533 -->

    <owl:NamedIndividual rdf:about="http://purl.obolibrary.org/obo/GAZ_00028533">
        <obo:RO_0001025 rdf:resource="http://purl.obolibrary.org/obo/GAZ_02000435"/>
        <oboInOwl:hasOBONamespace>GAZ</oboInOwl:hasOBONamespace>
        <oboInOwl:id>GAZ:00028533</oboInOwl:id>
        <rdfs:label>Municipality of Limassol</rdfs:label>
    </owl:NamedIndividual>
    


    <!-- http://purl.obolibrary.org/obo/GAZ_00028534 -->

    <owl:NamedIndividual rdf:about="http://purl.obolibrary.org/obo/GAZ_00028534">
        <obo:RO_0001025 rdf:resource="http://purl.obolibrary.org/obo/GAZ_02000435"/>
        <oboInOwl:hasOBONamespace>GAZ</oboInOwl:hasOBONamespace>
        <oboInOwl:id>GAZ:00028534</oboInOwl:id>
        <rdfs:label>Municipality of Kato Polemidia</rdfs:label>
    </owl:NamedIndividual>
    


    <!-- http://purl.obolibrary.org/obo/GAZ_00028535 -->

    <owl:NamedIndividual rdf:about="http://purl.obolibrary.org/obo/GAZ_00028535">
        <obo:RO_0001025 rdf:resource="http://purl.obolibrary.org/obo/GAZ_02000435"/>
        <oboInOwl:hasOBONamespace>GAZ</oboInOwl:hasOBONamespace>
        <oboInOwl:id>GAZ:00028535</oboInOwl:id>
        <rdfs:label>Municipality of Yermasoyia</rdfs:label>
    </owl:NamedIndividual>
    


    <!-- http://purl.obolibrary.org/obo/GAZ_00051148 -->

    <owl:NamedIndividual rdf:about="http://purl.obolibrary.org/obo/GAZ_00051148">
        <obo:RO_0001025 rdf:resource="http://purl.obolibrary.org/obo/GAZ_02000435"/>
        <obo:IAO_0000115>A saline lake located due south-east of the sprawling city of Limassol and measures 10.65 km2. Its lowest point is 2.7m below sea level and at its deepest point the water depth measures 1m.</obo:IAO_0000115>
        <oboInOwl:hasOBONamespace>GAZ</oboInOwl:hasOBONamespace>
        <oboInOwl:id>GAZ:00051148</oboInOwl:id>
        <rdfs:label>Limassol Salt Lake</rdfs:label>
    </owl:NamedIndividual>
    


    <!-- http://purl.obolibrary.org/obo/GAZ_00051149 -->

    <owl:NamedIndividual rdf:about="http://purl.obolibrary.org/obo/GAZ_00051149">
        <obo:RO_0001025 rdf:resource="http://purl.obolibrary.org/obo/GAZ_02000440"/>
        <obo:IAO_0000115>Salt lakes located to the west of the town of Larnaca. It is a complex network of four saline lakes (3 of them interconnected) of different sizes.</obo:IAO_0000115>
        <oboInOwl:hasOBONamespace>GAZ</oboInOwl:hasOBONamespace>
        <oboInOwl:id>GAZ:00051149</oboInOwl:id>
        <rdfs:label>Larnaca Salt Lakes</rdfs:label>
    </owl:NamedIndividual>
    


    <!-- http://purl.obolibrary.org/obo/GAZ_00051150 -->

    <owl:NamedIndividual rdf:about="http://purl.obolibrary.org/obo/GAZ_00051150">
        <obo:RO_0001025 rdf:resource="http://purl.obolibrary.org/obo/GAZ_00051149"/>
        <oboInOwl:hasOBONamespace>GAZ</oboInOwl:hasOBONamespace>
        <oboInOwl:id>GAZ:00051150</oboInOwl:id>
        <rdfs:label>Lake Orphani</rdfs:label>
    </owl:NamedIndividual>
    


    <!-- http://purl.obolibrary.org/obo/GAZ_00051151 -->

    <owl:NamedIndividual rdf:about="http://purl.obolibrary.org/obo/GAZ_00051151">
        <obo:RO_0001025 rdf:resource="http://purl.obolibrary.org/obo/GAZ_00051149"/>
        <oboInOwl:hasOBONamespace>GAZ</oboInOwl:hasOBONamespace>
        <oboInOwl:id>GAZ:00051151</oboInOwl:id>
        <rdfs:label>Lake Spiro</rdfs:label>
    </owl:NamedIndividual>
    


    <!-- http://purl.obolibrary.org/obo/GAZ_00051152 -->

    <owl:NamedIndividual rdf:about="http://purl.obolibrary.org/obo/GAZ_00051152">
        <obo:RO_0001025 rdf:resource="http://purl.obolibrary.org/obo/GAZ_00051149"/>
        <oboInOwl:hasOBONamespace>GAZ</oboInOwl:hasOBONamespace>
        <oboInOwl:id>GAZ:00051152</oboInOwl:id>
        <rdfs:label>Lake Soros</rdfs:label>
    </owl:NamedIndividual>
    


    <!-- http://purl.obolibrary.org/obo/GAZ_00051153 -->

    <owl:NamedIndividual rdf:about="http://purl.obolibrary.org/obo/GAZ_00051153">
        <obo:RO_0001025 rdf:resource="http://purl.obolibrary.org/obo/GAZ_00051149"/>
        <oboInOwl:hasOBONamespace>GAZ</oboInOwl:hasOBONamespace>
        <oboInOwl:id>GAZ:00051153</oboInOwl:id>
        <rdfs:label>Lake Aliki</rdfs:label>
    </owl:NamedIndividual>
    


    <!-- http://purl.obolibrary.org/obo/GAZ_00051348 -->

    <owl:NamedIndividual rdf:about="http://purl.obolibrary.org/obo/GAZ_00051348">
        <obo:RO_0001025 rdf:resource="http://purl.obolibrary.org/obo/GAZ_02000435"/>
        <obo:IAO_0000115>A bay on the south-western shore of the island of Cyprus, located between the cities of Paphos and Limassol in the Limassol District.</obo:IAO_0000115>
        <oboInOwl:hasOBONamespace>GAZ</oboInOwl:hasOBONamespace>
        <oboInOwl:id>GAZ:00051348</oboInOwl:id>
        <rdfs:label>Episkopi Bay</rdfs:label>
    </owl:NamedIndividual>
    


    <!-- http://purl.obolibrary.org/obo/GAZ_00051349 -->

    <owl:NamedIndividual rdf:about="http://purl.obolibrary.org/obo/GAZ_00051349">
        <obo:RO_0001025 rdf:resource="http://purl.obolibrary.org/obo/GAZ_02000437"/>
        <obo:IAO_0000115>A populated place. A village NE of Paphos.</obo:IAO_0000115>
        <oboInOwl:hasOBONamespace>GAZ</oboInOwl:hasOBONamespace>
        <oboInOwl:id>GAZ:00051349</oboInOwl:id>
        <rdfs:label>Episkopi</rdfs:label>
    </owl:NamedIndividual>
    


    <!-- http://purl.obolibrary.org/obo/GAZ_00051350 -->

    <owl:NamedIndividual rdf:about="http://purl.obolibrary.org/obo/GAZ_00051350">
        <rdf:type rdf:resource="http://purl.obolibrary.org/obo/ENVO_00000856"/>
        <obo:RO_0001025 rdf:resource="http://purl.obolibrary.org/obo/GAZ_02000439"/>
        <obo:IAO_0000115>A populated place. A village located 55 km south-west of the capital Nicosia on the north facing foothills of the Troodos Mountain range. It stands at an altitude of 667 m and it is the highest village in the Solea valley. It is surrounded by thick forestland and is built on the banks of the Kargotis and Garillis rivers. The two rivers join within village itself and form the river Klarios, which crosses the Solea valley and empties into Morfou Bay.</obo:IAO_0000115>
        <oboInOwl:hasOBONamespace>GAZ</oboInOwl:hasOBONamespace>
        <oboInOwl:id>GAZ:00051350</oboInOwl:id>
        <rdfs:label>Kakopetria</rdfs:label>
    </owl:NamedIndividual>
    


    <!-- http://purl.obolibrary.org/obo/GAZ_00051351 -->

    <owl:NamedIndividual rdf:about="http://purl.obolibrary.org/obo/GAZ_00051351">
        <obo:RO_0001025 rdf:resource="http://purl.obolibrary.org/obo/GAZ_00028491"/>
        <obo:IAO_0000115>A city on the east coast of Cyprus.</obo:IAO_0000115>
        <oboInOwl:hasOBONamespace>GAZ</oboInOwl:hasOBONamespace>
        <oboInOwl:id>GAZ:00051351</oboInOwl:id>
        <rdfs:label>Larnaca</rdfs:label>
    </owl:NamedIndividual>
    


    <!-- http://purl.obolibrary.org/obo/GAZ_00051352 -->

    <owl:NamedIndividual rdf:about="http://purl.obolibrary.org/obo/GAZ_00051352">
        <obo:RO_0001025 rdf:resource="http://purl.obolibrary.org/obo/GAZ_00028533"/>
        <obo:IAO_0000115>A city located on Akrotiri Bay, on the Cyrpus&apos;s southern coast and it is the capital of Limassol District.</obo:IAO_0000115>
        <oboInOwl:hasOBONamespace>GAZ</oboInOwl:hasOBONamespace>
        <oboInOwl:id>GAZ:00051352</oboInOwl:id>
        <rdfs:label>Limassol</rdfs:label>
    </owl:NamedIndividual>
    


    <!-- http://purl.obolibrary.org/obo/GAZ_00051354 -->

    <owl:NamedIndividual rdf:about="http://purl.obolibrary.org/obo/GAZ_00051354">
        <obo:RO_0001025 rdf:resource="http://purl.obolibrary.org/obo/GAZ_00028479"/>
        <obo:IAO_0000115>A coastal city in the southwest of Cyprus and the capital of Paphos District.</obo:IAO_0000115>
        <oboInOwl:hasOBONamespace>GAZ</oboInOwl:hasOBONamespace>
        <oboInOwl:id>GAZ:00051354</oboInOwl:id>
        <rdfs:label>Paphos</rdfs:label>
    </owl:NamedIndividual>
    


    <!-- http://purl.obolibrary.org/obo/GAZ_00051355 -->

    <owl:NamedIndividual rdf:about="http://purl.obolibrary.org/obo/GAZ_00051355">
        <rdf:type rdf:resource="http://purl.obolibrary.org/obo/ENVO_00000856"/>
        <obo:RO_0001025 rdf:resource="http://purl.obolibrary.org/obo/GAZ_00028482"/>
        <obo:IAO_0000115>A populated place. A town in Cyprus. It lies 12 km north of Paphos, in coastal hills inland from Coral Bay, at the southern end of the Akamas Peninsula.</obo:IAO_0000115>
        <oboInOwl:hasOBONamespace>GAZ</oboInOwl:hasOBONamespace>
        <oboInOwl:id>GAZ:00051355</oboInOwl:id>
        <rdfs:label>Peyia</rdfs:label>
    </owl:NamedIndividual>
    


    <!-- http://purl.obolibrary.org/obo/GAZ_00051356 -->

    <owl:NamedIndividual rdf:about="http://purl.obolibrary.org/obo/GAZ_00051356">
        <obo:RO_0001025 rdf:resource="http://purl.obolibrary.org/obo/GAZ_02000437"/>
        <obo:IAO_0000115>A peninsula at the northwest extremity of Cyprus.</obo:IAO_0000115>
        <oboInOwl:hasOBONamespace>GAZ</oboInOwl:hasOBONamespace>
        <oboInOwl:id>GAZ:00051356</oboInOwl:id>
        <rdfs:label>Akamas Peninsula</rdfs:label>
    </owl:NamedIndividual>
    


    <!-- http://purl.obolibrary.org/obo/GAZ_00051358 -->

    <owl:NamedIndividual rdf:about="http://purl.obolibrary.org/obo/GAZ_00051358">
        <rdf:type rdf:resource="http://purl.obolibrary.org/obo/ENVO_00000856"/>
        <obo:RO_0001025 rdf:resource="http://purl.obolibrary.org/obo/GAZ_00028481"/>
        <obo:IAO_0000115>A small town at the north-west end of the island of Cyprus, at the centre of Chrysochous Bay, and on the edge of the Akamas peninsula nature reserve.</obo:IAO_0000115>
        <oboInOwl:hasOBONamespace>GAZ</oboInOwl:hasOBONamespace>
        <oboInOwl:id>GAZ:00051358</oboInOwl:id>
        <rdfs:label>Polis</rdfs:label>
    </owl:NamedIndividual>
    


    <!-- http://purl.obolibrary.org/obo/GAZ_00051359 -->

    <owl:NamedIndividual rdf:about="http://purl.obolibrary.org/obo/GAZ_00051359">
        <obo:RO_0001025 rdf:resource="http://purl.obolibrary.org/obo/GAZ_02000440"/>
        <obo:IAO_0000115>A hill in Cyprus, on top of which stands a Greek Orthodox Monastery.</obo:IAO_0000115>
        <oboInOwl:hasOBONamespace>GAZ</oboInOwl:hasOBONamespace>
        <oboInOwl:id>GAZ:00051359</oboInOwl:id>
        <rdfs:label>Stavrovouni</rdfs:label>
    </owl:NamedIndividual>
    


    <!-- http://purl.obolibrary.org/obo/GAZ_00051361 -->

    <owl:NamedIndividual rdf:about="http://purl.obolibrary.org/obo/GAZ_00051361">
        <rdf:type rdf:resource="http://purl.obolibrary.org/obo/ENVO_00000856"/>
        <obo:RO_0001025 rdf:resource="http://purl.obolibrary.org/obo/GAZ_02000440"/>
        <obo:IAO_0000115>A small village located in the south of Cyprus between Limassol and Larnaca.</obo:IAO_0000115>
        <oboInOwl:hasOBONamespace>GAZ</oboInOwl:hasOBONamespace>
        <oboInOwl:id>GAZ:00051361</oboInOwl:id>
        <rdfs:label>Zygi</rdfs:label>
    </owl:NamedIndividual>
    


    <!-- http://purl.obolibrary.org/obo/GAZ_00051365 -->

    <owl:NamedIndividual rdf:about="http://purl.obolibrary.org/obo/GAZ_00051365">
        <obo:RO_0001025 rdf:resource="http://purl.obolibrary.org/obo/GAZ_02000437"/>
        <obo:IAO_0000115>A populated place. A village north of Paphos.</obo:IAO_0000115>
        <oboInOwl:hasOBONamespace>GAZ</oboInOwl:hasOBONamespace>
        <oboInOwl:id>GAZ:00051365</oboInOwl:id>
        <rdfs:label>Chloraka</rdfs:label>
    </owl:NamedIndividual>
    


    <!-- http://purl.obolibrary.org/obo/GAZ_00051370 -->

    <owl:NamedIndividual rdf:about="http://purl.obolibrary.org/obo/GAZ_00051370">
        <rdf:type rdf:resource="http://purl.obolibrary.org/obo/ENVO_00000856"/>
        <obo:RO_0001025 rdf:resource="http://purl.obolibrary.org/obo/GAZ_02000435"/>
        <obo:IAO_0000115>A populated place. A village on the outskirts of the city of Limassol, Cyprus. It is built close to the imposing castle which bears the settlement&apos;s name.</obo:IAO_0000115>
        <oboInOwl:hasOBONamespace>GAZ</oboInOwl:hasOBONamespace>
        <oboInOwl:id>GAZ:00051370</oboInOwl:id>
        <rdfs:label>Kolossi</rdfs:label>
    </owl:NamedIndividual>
    


    <!-- http://purl.obolibrary.org/obo/GAZ_00051371 -->

    <owl:NamedIndividual rdf:about="http://purl.obolibrary.org/obo/GAZ_00051371">
        <obo:RO_0001025 rdf:resource="http://purl.obolibrary.org/obo/GAZ_00051370"/>
        <obo:IAO_0000115>A stronghold a few km outside the city of Limassol on the island of Cyprus.</obo:IAO_0000115>
        <oboInOwl:hasOBONamespace>GAZ</oboInOwl:hasOBONamespace>
        <oboInOwl:id>GAZ:00051371</oboInOwl:id>
        <rdfs:label>Kolossi Castle</rdfs:label>
    </owl:NamedIndividual>
    


    <!-- http://purl.obolibrary.org/obo/GAZ_00051372 -->

    <owl:NamedIndividual rdf:about="http://purl.obolibrary.org/obo/GAZ_00051372">
        <obo:RO_0001025 rdf:resource="http://purl.obolibrary.org/obo/GAZ_02000437"/>
        <oboInOwl:hasOBONamespace>GAZ</oboInOwl:hasOBONamespace>
        <oboInOwl:id>GAZ:00051372</oboInOwl:id>
        <rdfs:label>Paphos Forest</rdfs:label>
    </owl:NamedIndividual>
    


    <!-- http://purl.obolibrary.org/obo/GAZ_00051373 -->

    <owl:NamedIndividual rdf:about="http://purl.obolibrary.org/obo/GAZ_00051373">
        <obo:RO_0001025 rdf:resource="http://purl.obolibrary.org/obo/GAZ_02000437"/>
        <oboInOwl:hasOBONamespace>GAZ</oboInOwl:hasOBONamespace>
        <oboInOwl:id>GAZ:00051373</oboInOwl:id>
        <rdfs:label>Stavros tis Psokas River</rdfs:label>
    </owl:NamedIndividual>
    


    <!-- http://purl.obolibrary.org/obo/GAZ_00051376 -->

    <owl:NamedIndividual rdf:about="http://purl.obolibrary.org/obo/GAZ_00051376">
        <obo:RO_0001025 rdf:resource="http://purl.obolibrary.org/obo/GAZ_02000437"/>
        <oboInOwl:hasOBONamespace>GAZ</oboInOwl:hasOBONamespace>
        <oboInOwl:id>GAZ:00051376</oboInOwl:id>
        <rdfs:label>Khrysokhou Bay</rdfs:label>
    </owl:NamedIndividual>
    


    <!-- http://purl.obolibrary.org/obo/GAZ_00051377 -->

    <owl:NamedIndividual rdf:about="http://purl.obolibrary.org/obo/GAZ_00051377">
        <obo:RO_0001025 rdf:resource="http://purl.obolibrary.org/obo/GAZ_02000437"/>
        <obo:IAO_0000115>Officially comprised of two villages, the larger Kato Pyrgos and the smaller Pano Pyrgos; located on the Morphou Bay and surrounded by the Troodos Mountains.</obo:IAO_0000115>
        <oboInOwl:hasOBONamespace>GAZ</oboInOwl:hasOBONamespace>
        <oboInOwl:id>GAZ:00051377</oboInOwl:id>
        <rdfs:label>Pyrgos</rdfs:label>
    </owl:NamedIndividual>
    


    <!-- http://purl.obolibrary.org/obo/GAZ_00051378 -->

    <owl:NamedIndividual rdf:about="http://purl.obolibrary.org/obo/GAZ_00051378">
        <obo:RO_0001025 rdf:resource="http://purl.obolibrary.org/obo/GAZ_00051377"/>
        <oboInOwl:hasOBONamespace>GAZ</oboInOwl:hasOBONamespace>
        <oboInOwl:id>GAZ:00051378</oboInOwl:id>
        <rdfs:label>Kato Pyrgos</rdfs:label>
    </owl:NamedIndividual>
    


    <!-- http://purl.obolibrary.org/obo/GAZ_00051379 -->

    <owl:NamedIndividual rdf:about="http://purl.obolibrary.org/obo/GAZ_00051379">
        <obo:RO_0001025 rdf:resource="http://purl.obolibrary.org/obo/GAZ_00051377"/>
        <oboInOwl:hasOBONamespace>GAZ</oboInOwl:hasOBONamespace>
        <oboInOwl:id>GAZ:00051379</oboInOwl:id>
        <rdfs:label>Pano Pyrgos</rdfs:label>
    </owl:NamedIndividual>
    


    <!-- http://purl.obolibrary.org/obo/GAZ_00228439 -->

    <owl:NamedIndividual rdf:about="http://purl.obolibrary.org/obo/GAZ_00228439">
        <rdf:type rdf:resource="http://purl.obolibrary.org/obo/ENVO_00000856"/>
        <obo:RO_0001025 rdf:resource="http://purl.obolibrary.org/obo/GAZ_02000440"/>
        <obo:IAO_0000115>A populated place. A village in Larnaca District in south-eastern Cyprus. An enclave in the Eastern Sovereign Base Area.</obo:IAO_0000115>
        <oboInOwl:hasOBONamespace>GAZ</oboInOwl:hasOBONamespace>
        <oboInOwl:id>GAZ:00228439</oboInOwl:id>
        <rdfs:label>Xylotymvou</rdfs:label>
    </owl:NamedIndividual>
    


    <!-- http://purl.obolibrary.org/obo/GAZ_00228440 -->

    <owl:NamedIndividual rdf:about="http://purl.obolibrary.org/obo/GAZ_00228440">
        <rdf:type rdf:resource="http://purl.obolibrary.org/obo/ENVO_00000856"/>
        <obo:RO_0001025 rdf:resource="http://purl.obolibrary.org/obo/GAZ_02000440"/>
        <obo:IAO_0000115>A populated place. A village in Larnaca District in south-eastern Cyprus. An enclave in the Eastern Sovereign Base Area.</obo:IAO_0000115>
        <oboInOwl:hasOBONamespace>GAZ</oboInOwl:hasOBONamespace>
        <oboInOwl:id>GAZ:00228440</oboInOwl:id>
        <rdfs:label>Ormideia</rdfs:label>
    </owl:NamedIndividual>
    


    <!-- http://purl.obolibrary.org/obo/GAZ_00358443 -->

    <owl:NamedIndividual rdf:about="http://purl.obolibrary.org/obo/GAZ_00358443">
        <obo:RO_0001025 rdf:resource="http://purl.obolibrary.org/obo/GAZ_00051356"/>
        <obo:IAO_0000115>A bay on the Akamas Peninsula.</obo:IAO_0000115>
        <oboInOwl:hasOBONamespace>GAZ</oboInOwl:hasOBONamespace>
        <oboInOwl:id>GAZ:00358443</oboInOwl:id>
        <rdfs:label>Fontana Amorosa</rdfs:label>
    </owl:NamedIndividual>
    


    <!-- http://purl.obolibrary.org/obo/GAZ_00358444 -->

    <owl:NamedIndividual rdf:about="http://purl.obolibrary.org/obo/GAZ_00358444">
        <obo:RO_0001025 rdf:resource="http://purl.obolibrary.org/obo/GAZ_02000435"/>
        <obo:IAO_0000115>A dam. Completed 1968.</obo:IAO_0000115>
        <oboInOwl:hasOBONamespace>GAZ</oboInOwl:hasOBONamespace>
        <oboInOwl:id>GAZ:00358444</oboInOwl:id>
        <rdfs:label>Kouris Dam</rdfs:label>
    </owl:NamedIndividual>
    


    <!-- http://purl.obolibrary.org/obo/GAZ_00358445 -->

    <owl:NamedIndividual rdf:about="http://purl.obolibrary.org/obo/GAZ_00358445">
        <obo:RO_0001025 rdf:resource="http://purl.obolibrary.org/obo/GAZ_02000437"/>
        <obo:IAO_0000115>A dam. Completed 1978-05.</obo:IAO_0000115>
        <oboInOwl:hasOBONamespace>GAZ</oboInOwl:hasOBONamespace>
        <oboInOwl:id>GAZ:00358445</oboInOwl:id>
        <rdfs:label>Asprokremmos Dam</rdfs:label>
    </owl:NamedIndividual>
    


    <!-- http://purl.obolibrary.org/obo/GAZ_00358446 -->

    <owl:NamedIndividual rdf:about="http://purl.obolibrary.org/obo/GAZ_00358446">
        <obo:RO_0001025 rdf:resource="http://purl.obolibrary.org/obo/GAZ_02000437"/>
        <obo:IAO_0000115>A dam. Completed 1986.</obo:IAO_0000115>
        <oboInOwl:hasOBONamespace>GAZ</oboInOwl:hasOBONamespace>
        <oboInOwl:id>GAZ:00358446</oboInOwl:id>
        <rdfs:label>Evretou Dam</rdfs:label>
    </owl:NamedIndividual>
    


    <!-- http://purl.obolibrary.org/obo/GAZ_00358447 -->

    <owl:NamedIndividual rdf:about="http://purl.obolibrary.org/obo/GAZ_00358447">
        <obo:RO_0001025 rdf:resource="http://purl.obolibrary.org/obo/GAZ_02000437"/>
        <obo:IAO_0000115>A dam. Completed 2005.</obo:IAO_0000115>
        <oboInOwl:hasOBONamespace>GAZ</oboInOwl:hasOBONamespace>
        <oboInOwl:id>GAZ:00358447</oboInOwl:id>
        <rdfs:label>Kannaviou Dam</rdfs:label>
    </owl:NamedIndividual>
    


    <!-- http://purl.obolibrary.org/obo/GAZ_00358448 -->

    <owl:NamedIndividual rdf:about="http://purl.obolibrary.org/obo/GAZ_00358448">
        <obo:RO_0001025 rdf:resource="http://purl.obolibrary.org/obo/GAZ_02000439"/>
        <obo:IAO_0000115>A dam. Completed 2002.</obo:IAO_0000115>
        <oboInOwl:hasOBONamespace>GAZ</oboInOwl:hasOBONamespace>
        <oboInOwl:id>GAZ:00358448</oboInOwl:id>
        <rdfs:label>Tamasos Dam</rdfs:label>
    </owl:NamedIndividual>
    


    <!-- http://purl.obolibrary.org/obo/GAZ_00358449 -->

    <owl:NamedIndividual rdf:about="http://purl.obolibrary.org/obo/GAZ_00358449">
        <obo:RO_0001025 rdf:resource="http://purl.obolibrary.org/obo/GAZ_02000435"/>
        <obo:IAO_0000115>A dam. Completed 1968.</obo:IAO_0000115>
        <oboInOwl:hasOBONamespace>GAZ</oboInOwl:hasOBONamespace>
        <oboInOwl:id>GAZ:00358449</oboInOwl:id>
        <rdfs:label>Yermasoyia Dam</rdfs:label>
    </owl:NamedIndividual>
    


    <!-- http://purl.obolibrary.org/obo/GAZ_00358450 -->

    <owl:NamedIndividual rdf:about="http://purl.obolibrary.org/obo/GAZ_00358450">
        <obo:RO_0001025 rdf:resource="http://purl.obolibrary.org/obo/GAZ_02000440"/>
        <obo:IAO_0000115>A dam.</obo:IAO_0000115>
        <oboInOwl:hasOBONamespace>GAZ</oboInOwl:hasOBONamespace>
        <oboInOwl:id>GAZ:00358450</oboInOwl:id>
        <rdfs:label>Kalavasos Dam</rdfs:label>
    </owl:NamedIndividual>
    


    <!-- http://purl.obolibrary.org/obo/GAZ_00358451 -->

    <owl:NamedIndividual rdf:about="http://purl.obolibrary.org/obo/GAZ_00358451">
        <obo:RO_0001025 rdf:resource="http://purl.obolibrary.org/obo/GAZ_02000440"/>
        <obo:IAO_0000115>A dam.</obo:IAO_0000115>
        <oboInOwl:hasOBONamespace>GAZ</oboInOwl:hasOBONamespace>
        <oboInOwl:id>GAZ:00358451</oboInOwl:id>
        <rdfs:label>Dipotamos Dam</rdfs:label>
    </owl:NamedIndividual>
    


    <!-- http://purl.obolibrary.org/obo/GAZ_00358452 -->

    <owl:NamedIndividual rdf:about="http://purl.obolibrary.org/obo/GAZ_00358452">
        <obo:RO_0001025 rdf:resource="http://purl.obolibrary.org/obo/GAZ_02000440"/>
        <obo:IAO_0000115>A dam.</obo:IAO_0000115>
        <oboInOwl:hasOBONamespace>GAZ</oboInOwl:hasOBONamespace>
        <oboInOwl:id>GAZ:00358452</oboInOwl:id>
        <rdfs:label>Lefkara Dam</rdfs:label>
    </owl:NamedIndividual>
    


    <!-- http://purl.obolibrary.org/obo/GAZ_00358453 -->

    <owl:NamedIndividual rdf:about="http://purl.obolibrary.org/obo/GAZ_00358453">
        <obo:IAO_0000115>A river in Cyprus. The river originates in the Troodos Mountains close to Machairas Monastery and flows northeast across the Mesaoria plains, through the capital city Nicosia. It then steers east, meeting the sea at Famagusta Bay close to the ancient Greek city of Salamis.</obo:IAO_0000115>
        <oboInOwl:hasOBONamespace>GAZ</oboInOwl:hasOBONamespace>
        <oboInOwl:id>GAZ:00358453</oboInOwl:id>
        <rdfs:label>Pedieos</rdfs:label>
    </owl:NamedIndividual>
    


    <!-- http://purl.obolibrary.org/obo/GAZ_00358454 -->

    <owl:NamedIndividual rdf:about="http://purl.obolibrary.org/obo/GAZ_00358454">
        <obo:RO_0001025 rdf:resource="http://purl.obolibrary.org/obo/GAZ_02000435"/>
        <obo:IAO_0000115>An archeological site. Arock shelter near Limassol on the southern coast of Cyprus. It is situated on a steep cliff site ca. 40m above the Mediterranean.</obo:IAO_0000115>
        <oboInOwl:hasOBONamespace>GAZ</oboInOwl:hasOBONamespace>
        <oboInOwl:id>GAZ:00358454</oboInOwl:id>
        <rdfs:label>Aetokremnos</rdfs:label>
    </owl:NamedIndividual>
    


    <!-- http://purl.obolibrary.org/obo/GAZ_00358455 -->

    <owl:NamedIndividual rdf:about="http://purl.obolibrary.org/obo/GAZ_00358455">
        <obo:RO_0001025 rdf:resource="http://purl.obolibrary.org/obo/GAZ_02000435"/>
        <obo:IAO_0000115>An archeological site. A former city located on the southern coast in front of Agios Tychonas, about 24 miles west of Larnaca and 6 miles east of Limassol.</obo:IAO_0000115>
        <oboInOwl:hasOBONamespace>GAZ</oboInOwl:hasOBONamespace>
        <oboInOwl:id>GAZ:00358455</oboInOwl:id>
        <rdfs:label>Amathus</rdfs:label>
    </owl:NamedIndividual>
    


    <!-- http://purl.obolibrary.org/obo/GAZ_00358456 -->

    <owl:NamedIndividual rdf:about="http://purl.obolibrary.org/obo/GAZ_00358456">
        <obo:RO_0001025 rdf:resource="http://purl.obolibrary.org/obo/GAZ_02000440"/>
        <obo:IAO_0000115>An archaeological site on the island of Cyprus dating from the Neolithic age.</obo:IAO_0000115>
        <oboInOwl:hasOBONamespace>GAZ</oboInOwl:hasOBONamespace>
        <oboInOwl:id>GAZ:00358456</oboInOwl:id>
        <rdfs:label>Khirokitia</rdfs:label>
    </owl:NamedIndividual>
    


    <!-- http://purl.obolibrary.org/obo/GAZ_00358457 -->

    <owl:NamedIndividual rdf:about="http://purl.obolibrary.org/obo/GAZ_00358457">
        <obo:RO_0001025 rdf:resource="http://purl.obolibrary.org/obo/GAZ_02000440"/>
        <obo:IAO_0000115>An archeological site. A former city in Cyprus, which endured from antiquity until the early Middle Ages.</obo:IAO_0000115>
        <oboInOwl:hasOBONamespace>GAZ</oboInOwl:hasOBONamespace>
        <oboInOwl:id>GAZ:00358457</oboInOwl:id>
        <rdfs:label>Kourion</rdfs:label>
    </owl:NamedIndividual>
    


    <!-- http://purl.obolibrary.org/obo/GAZ_00358460 -->

    <owl:NamedIndividual rdf:about="http://purl.obolibrary.org/obo/GAZ_00358460">
        <obo:RO_0001025 rdf:resource="http://purl.obolibrary.org/obo/GAZ_02000437"/>
        <obo:IAO_0000115>An archeological site. Located near to the present town of Polis</obo:IAO_0000115>
        <oboInOwl:hasOBONamespace>GAZ</oboInOwl:hasOBONamespace>
        <oboInOwl:id>GAZ:00358460</oboInOwl:id>
        <rdfs:label>Marion</rdfs:label>
    </owl:NamedIndividual>
    


    <!-- http://purl.obolibrary.org/obo/GAZ_00358461 -->

    <owl:NamedIndividual rdf:about="http://purl.obolibrary.org/obo/GAZ_00358461">
        <obo:RO_0001025 rdf:resource="http://purl.obolibrary.org/obo/GAZ_02000435"/>
        <obo:IAO_0000115>An archeological site. Neolithic.</obo:IAO_0000115>
        <oboInOwl:hasOBONamespace>GAZ</oboInOwl:hasOBONamespace>
        <oboInOwl:id>GAZ:00358461</oboInOwl:id>
        <rdfs:label>Shillourokambos</rdfs:label>
    </owl:NamedIndividual>
    


    <!-- http://purl.obolibrary.org/obo/GAZ_00358462 -->

    <owl:NamedIndividual rdf:about="http://purl.obolibrary.org/obo/GAZ_00358462">
        <obo:RO_0001025 rdf:resource="http://purl.obolibrary.org/obo/GAZ_02000440"/>
        <obo:IAO_0000115>An archeological site.</obo:IAO_0000115>
        <oboInOwl:hasOBONamespace>GAZ</oboInOwl:hasOBONamespace>
        <oboInOwl:id>GAZ:00358462</oboInOwl:id>
        <rdfs:label>Tenta</rdfs:label>
    </owl:NamedIndividual>
    


    <!-- http://purl.obolibrary.org/obo/GAZ_00358463 -->

    <owl:NamedIndividual rdf:about="http://purl.obolibrary.org/obo/GAZ_00358463">
        <obo:RO_0001025 rdf:resource="http://purl.obolibrary.org/obo/GAZ_00028479"/>
        <obo:IAO_0000115>An archeological site. A large necropolis lying about two km north-west of Paphos harbour in Cyprus.</obo:IAO_0000115>
        <oboInOwl:hasOBONamespace>GAZ</oboInOwl:hasOBONamespace>
        <oboInOwl:id>GAZ:00358463</oboInOwl:id>
        <rdfs:label>Tombs of the Kings</rdfs:label>
    </owl:NamedIndividual>
    


    <!-- http://purl.obolibrary.org/obo/GAZ_02000434 -->

    <owl:NamedIndividual rdf:about="http://purl.obolibrary.org/obo/GAZ_02000434">
        <obo:RO_0001025 rdf:resource="http://purl.obolibrary.org/obo/GAZ_00004007"/>
    </owl:NamedIndividual>
    


    <!-- http://purl.obolibrary.org/obo/GAZ_02000435 -->

    <owl:NamedIndividual rdf:about="http://purl.obolibrary.org/obo/GAZ_02000435"/>
    


    <!-- http://purl.obolibrary.org/obo/GAZ_02000436 -->

    <owl:NamedIndividual rdf:about="http://purl.obolibrary.org/obo/GAZ_02000436"/>
    


    <!-- http://purl.obolibrary.org/obo/GAZ_02000437 -->

    <owl:NamedIndividual rdf:about="http://purl.obolibrary.org/obo/GAZ_02000437"/>
    


    <!-- http://purl.obolibrary.org/obo/GAZ_02000439 -->

    <owl:NamedIndividual rdf:about="http://purl.obolibrary.org/obo/GAZ_02000439"/>
    


    <!-- http://purl.obolibrary.org/obo/GAZ_02000440 -->

    <owl:NamedIndividual rdf:about="http://purl.obolibrary.org/obo/GAZ_02000440"/>
    


    <!-- 
    ///////////////////////////////////////////////////////////////////////////////////////
    //
    // Annotations
    //
    ///////////////////////////////////////////////////////////////////////////////////////
     -->

    <rdf:Description rdf:about="http://purl.obolibrary.org/obo/GAZ_02000434">
        <rdfs:label>District (Republic of Cyprus)</rdfs:label>
        <oboInOwl:id>GAZ:02000434</oboInOwl:id>
        <oboInOwl:hasOBONamespace>GAZ</oboInOwl:hasOBONamespace>
    </rdf:Description>
    <rdf:Description rdf:about="http://purl.obolibrary.org/obo/GAZ_02000435">
        <obo:IAO_0000115>One of the six districts of Cyprus. Part of the British overseas territory of Akrotiri and Dhekelia forms an enclave on the Akrotiri peninsula, under the sovereignty of the United Kingdom.</obo:IAO_0000115>
        <oboInOwl:id>GAZ:02000435</oboInOwl:id>
        <oboInOwl:hasOBONamespace>GAZ</oboInOwl:hasOBONamespace>
        <rdfs:label>Limassol District</rdfs:label>
    </rdf:Description>
    <rdf:Description rdf:about="http://purl.obolibrary.org/obo/GAZ_02000436">
        <oboInOwl:hasOBONamespace>GAZ</oboInOwl:hasOBONamespace>
        <rdfs:label>Famagusta District</rdfs:label>
        <obo:IAO_0000115>One of the six districts of Cyprus. Most of the district has been under Turkish control since the 1974 invasion. Since then, the northeastern section, including the Karpasia Peninsula, has been administered separately as the Iskele District, a division not recognized by the Republic of Cyprus.</obo:IAO_0000115>
        <oboInOwl:id>GAZ:02000436</oboInOwl:id>
    </rdf:Description>
    <rdf:Description rdf:about="http://purl.obolibrary.org/obo/GAZ_02000437">
        <oboInOwl:hasOBONamespace>GAZ</oboInOwl:hasOBONamespace>
        <oboInOwl:id>GAZ:02000437</oboInOwl:id>
        <obo:IAO_0000115>One of the six districts of Cyprus and it is situated in the western part of Cyprus.</obo:IAO_0000115>
        <rdfs:label>Paphos District</rdfs:label>
    </rdf:Description>
    <rdf:Description rdf:about="http://purl.obolibrary.org/obo/GAZ_02000439">
        <oboInOwl:hasOBONamespace>GAZ</oboInOwl:hasOBONamespace>
        <oboInOwl:id>GAZ:02000439</oboInOwl:id>
        <obo:IAO_0000115>One of the six districts of Cyprus. Its main town is the island country&apos;s capital city, Nicosia. The Turkish-occupied northern part of the city is the capital of the so called Turkish Republic of Northern Cyprus.</obo:IAO_0000115>
        <rdfs:label>Nicosia District</rdfs:label>
    </rdf:Description>
    <rdf:Description rdf:about="http://purl.obolibrary.org/obo/GAZ_02000440">
        <rdfs:label>Larnaca District</rdfs:label>
        <oboInOwl:hasOBONamespace>GAZ</oboInOwl:hasOBONamespace>
        <oboInOwl:id>GAZ:02000440</oboInOwl:id>
        <obo:IAO_0000115>One of the six districts of Cyprus. The authorities in Turkish Republic of Northern Cyprus administer the Turkish-occupied parts of Larnaca District as part of Nicosia District.</obo:IAO_0000115>
    </rdf:Description>
</rdf:RDF>



<!-- Generated by the OWL API (version 4.5.6) https://github.com/owlcs/owlapi -->

