<?xml version="1.0"?>
<rdf:RDF xmlns="http://purl.obolibrary.org/obo/gaz/subsets/countries/Republic_of_South_Africa.owl#"
     xml:base="http://purl.obolibrary.org/obo/gaz/subsets/countries/Republic_of_South_Africa.owl"
     xmlns:obo="http://purl.obolibrary.org/obo/"
     xmlns:owl="http://www.w3.org/2002/07/owl#"
     xmlns:rdf="http://www.w3.org/1999/02/22-rdf-syntax-ns#"
     xmlns:xml="http://www.w3.org/XML/1998/namespace"
     xmlns:xsd="http://www.w3.org/2001/XMLSchema#"
     xmlns:rdfs="http://www.w3.org/2000/01/rdf-schema#"
     xmlns:oboInOwl="http://www.geneontology.org/formats/oboInOwl#">
    <owl:Ontology rdf:about="http://purl.obolibrary.org/obo/gaz/subsets/countries/Republic_of_South_Africa.owl">
        <owl:imports rdf:resource="http://purl.obolibrary.org/obo/gaz/imports/envo_import.owl"/>
        <owl:imports rdf:resource="http://purl.obolibrary.org/obo/gaz/imports/ro_import.owl"/>
    </owl:Ontology>
    


    <!-- 
    ///////////////////////////////////////////////////////////////////////////////////////
    //
    // Annotation properties
    //
    ///////////////////////////////////////////////////////////////////////////////////////
     -->

    


    <!-- http://purl.obolibrary.org/obo/IAO_0000115 -->

    <owl:AnnotationProperty rdf:about="http://purl.obolibrary.org/obo/IAO_0000115"/>
    


    <!-- http://www.geneontology.org/formats/oboInOwl#hasOBONamespace -->

    <owl:AnnotationProperty rdf:about="http://www.geneontology.org/formats/oboInOwl#hasOBONamespace"/>
    


    <!-- http://www.geneontology.org/formats/oboInOwl#id -->

    <owl:AnnotationProperty rdf:about="http://www.geneontology.org/formats/oboInOwl#id"/>
    


    <!-- 
    ///////////////////////////////////////////////////////////////////////////////////////
    //
    // Object Properties
    //
    ///////////////////////////////////////////////////////////////////////////////////////
     -->

    


    <!-- http://purl.obolibrary.org/obo/RO_0001025 -->

    <owl:ObjectProperty rdf:about="http://purl.obolibrary.org/obo/RO_0001025"/>
    


    <!-- 
    ///////////////////////////////////////////////////////////////////////////////////////
    //
    // Classes
    //
    ///////////////////////////////////////////////////////////////////////////////////////
     -->

    


    <!-- http://purl.obolibrary.org/obo/ENVO_00000004 -->

    <owl:Class rdf:about="http://purl.obolibrary.org/obo/ENVO_00000004"/>
    


    <!-- http://purl.obolibrary.org/obo/ENVO_00000009 -->

    <owl:Class rdf:about="http://purl.obolibrary.org/obo/ENVO_00000009"/>
    


    <!-- http://purl.obolibrary.org/obo/ENVO_00000100 -->

    <owl:Class rdf:about="http://purl.obolibrary.org/obo/ENVO_00000100"/>
    


    <!-- http://purl.obolibrary.org/obo/ENVO_00000106 -->

    <owl:Class rdf:about="http://purl.obolibrary.org/obo/ENVO_00000106"/>
    


    <!-- http://purl.obolibrary.org/obo/ENVO_00000191 -->

    <owl:Class rdf:about="http://purl.obolibrary.org/obo/ENVO_00000191"/>
    


    <!-- http://purl.obolibrary.org/obo/ENVO_00000220 -->

    <owl:Class rdf:about="http://purl.obolibrary.org/obo/ENVO_00000220"/>
    


    <!-- http://purl.obolibrary.org/obo/ENVO_00000305 -->

    <owl:Class rdf:about="http://purl.obolibrary.org/obo/ENVO_00000305"/>
    


    <!-- http://purl.obolibrary.org/obo/ENVO_00000309 -->

    <owl:Class rdf:about="http://purl.obolibrary.org/obo/ENVO_00000309"/>
    


    <!-- http://purl.obolibrary.org/obo/ENVO_00000856 -->

    <owl:Class rdf:about="http://purl.obolibrary.org/obo/ENVO_00000856"/>
    


    <!-- http://purl.obolibrary.org/obo/GAZ_00002810 -->

    <owl:Class rdf:about="http://purl.obolibrary.org/obo/GAZ_00002810"/>
    


    <!-- http://purl.obolibrary.org/obo/GAZ_00002811 -->

    <owl:Class rdf:about="http://purl.obolibrary.org/obo/GAZ_00002811">
        <rdfs:subClassOf rdf:resource="http://purl.obolibrary.org/obo/GAZ_00002810"/>
    </owl:Class>
    


    <!-- http://purl.obolibrary.org/obo/GAZ_00002812 -->

    <owl:Class rdf:about="http://purl.obolibrary.org/obo/GAZ_00002812">
        <rdfs:subClassOf rdf:resource="http://purl.obolibrary.org/obo/GAZ_00002810"/>
    </owl:Class>
    


    <!-- http://purl.obolibrary.org/obo/GAZ_00002813 -->

    <owl:Class rdf:about="http://purl.obolibrary.org/obo/GAZ_00002813">
        <rdfs:subClassOf rdf:resource="http://purl.obolibrary.org/obo/GAZ_00002810"/>
    </owl:Class>
    


    <!-- http://purl.obolibrary.org/obo/GAZ_00002814 -->

    <owl:Class rdf:about="http://purl.obolibrary.org/obo/GAZ_00002814">
        <rdfs:subClassOf rdf:resource="http://purl.obolibrary.org/obo/GAZ_00002810"/>
    </owl:Class>
    


    <!-- http://purl.obolibrary.org/obo/GAZ_00002815 -->

    <owl:Class rdf:about="http://purl.obolibrary.org/obo/GAZ_00002815">
        <rdfs:subClassOf rdf:resource="http://purl.obolibrary.org/obo/GAZ_00002810"/>
    </owl:Class>
    


    <!-- http://purl.obolibrary.org/obo/GAZ_00002816 -->

    <owl:Class rdf:about="http://purl.obolibrary.org/obo/GAZ_00002816">
        <rdfs:subClassOf rdf:resource="http://purl.obolibrary.org/obo/GAZ_00002810"/>
    </owl:Class>
    


    <!-- http://purl.obolibrary.org/obo/GAZ_00002817 -->

    <owl:Class rdf:about="http://purl.obolibrary.org/obo/GAZ_00002817">
        <rdfs:subClassOf rdf:resource="http://purl.obolibrary.org/obo/GAZ_00002810"/>
    </owl:Class>
    


    <!-- http://purl.obolibrary.org/obo/GAZ_00002818 -->

    <owl:Class rdf:about="http://purl.obolibrary.org/obo/GAZ_00002818">
        <rdfs:subClassOf rdf:resource="http://purl.obolibrary.org/obo/GAZ_00002810"/>
    </owl:Class>
    


    <!-- http://purl.obolibrary.org/obo/GAZ_00002819 -->

    <owl:Class rdf:about="http://purl.obolibrary.org/obo/GAZ_00002819">
        <rdfs:subClassOf rdf:resource="http://purl.obolibrary.org/obo/GAZ_00002810"/>
    </owl:Class>
    


    <!-- http://purl.obolibrary.org/obo/GAZ_00003034 -->

    <owl:Class rdf:about="http://purl.obolibrary.org/obo/GAZ_00003034"/>
    


    <!-- http://purl.obolibrary.org/obo/GAZ_00003035 -->

    <owl:Class rdf:about="http://purl.obolibrary.org/obo/GAZ_00003035">
        <rdfs:subClassOf rdf:resource="http://purl.obolibrary.org/obo/GAZ_00003034"/>
    </owl:Class>
    


    <!-- http://purl.obolibrary.org/obo/GAZ_00003725 -->

    <owl:Class rdf:about="http://purl.obolibrary.org/obo/GAZ_00003725">
        <rdfs:subClassOf rdf:resource="http://purl.obolibrary.org/obo/GAZ_00003034"/>
    </owl:Class>
    


    <!-- http://purl.obolibrary.org/obo/GAZ_00003726 -->

    <owl:Class rdf:about="http://purl.obolibrary.org/obo/GAZ_00003726">
        <rdfs:subClassOf rdf:resource="http://purl.obolibrary.org/obo/GAZ_00003034"/>
    </owl:Class>
    


    <!-- http://purl.obolibrary.org/obo/GAZ_00005305 -->

    <owl:Class rdf:about="http://purl.obolibrary.org/obo/GAZ_00005305">
        <rdfs:subClassOf rdf:resource="http://purl.obolibrary.org/obo/GAZ_00003034"/>
    </owl:Class>
    


    <!-- http://purl.obolibrary.org/obo/GAZ_00005306 -->

    <owl:Class rdf:about="http://purl.obolibrary.org/obo/GAZ_00005306">
        <rdfs:subClassOf rdf:resource="http://purl.obolibrary.org/obo/GAZ_00003034"/>
    </owl:Class>
    


    <!-- http://purl.obolibrary.org/obo/GAZ_00005310 -->

    <owl:Class rdf:about="http://purl.obolibrary.org/obo/GAZ_00005310">
        <rdfs:subClassOf rdf:resource="http://purl.obolibrary.org/obo/GAZ_00003034"/>
    </owl:Class>
    


    <!-- http://purl.obolibrary.org/obo/GAZ_00005311 -->

    <owl:Class rdf:about="http://purl.obolibrary.org/obo/GAZ_00005311">
        <rdfs:subClassOf rdf:resource="http://purl.obolibrary.org/obo/GAZ_00003034"/>
    </owl:Class>
    


    <!-- http://purl.obolibrary.org/obo/GAZ_00005314 -->

    <owl:Class rdf:about="http://purl.obolibrary.org/obo/GAZ_00005314">
        <rdfs:subClassOf rdf:resource="http://purl.obolibrary.org/obo/GAZ_00003034"/>
    </owl:Class>
    


    <!-- http://purl.obolibrary.org/obo/GAZ_00005316 -->

    <owl:Class rdf:about="http://purl.obolibrary.org/obo/GAZ_00005316">
        <rdfs:subClassOf rdf:resource="http://purl.obolibrary.org/obo/GAZ_00003034"/>
    </owl:Class>
    


    <!-- http://purl.obolibrary.org/obo/GAZ_00008041 -->

    <owl:Class rdf:about="http://purl.obolibrary.org/obo/GAZ_00008041">
        <rdfs:subClassOf rdf:resource="http://purl.obolibrary.org/obo/GAZ_00003034"/>
    </owl:Class>
    


    <!-- http://purl.obolibrary.org/obo/GAZ_00010007 -->

    <owl:Class rdf:about="http://purl.obolibrary.org/obo/GAZ_00010007">
        <rdfs:subClassOf rdf:resource="http://purl.obolibrary.org/obo/GAZ_00003034"/>
    </owl:Class>
    


    <!-- http://purl.obolibrary.org/obo/GAZ_00010008 -->

    <owl:Class rdf:about="http://purl.obolibrary.org/obo/GAZ_00010008">
        <rdfs:subClassOf rdf:resource="http://purl.obolibrary.org/obo/GAZ_00003034"/>
    </owl:Class>
    


    <!-- http://purl.obolibrary.org/obo/GAZ_00052064 -->

    <owl:Class rdf:about="http://purl.obolibrary.org/obo/GAZ_00052064">
        <rdfs:subClassOf rdf:resource="http://purl.obolibrary.org/obo/GAZ_00003034"/>
    </owl:Class>
    


    <!-- http://purl.obolibrary.org/obo/GAZ_00052087 -->

    <owl:Class rdf:about="http://purl.obolibrary.org/obo/GAZ_00052087">
        <rdfs:subClassOf rdf:resource="http://purl.obolibrary.org/obo/GAZ_00003034"/>
    </owl:Class>
    


    <!-- http://purl.obolibrary.org/obo/GAZ_00052090 -->

    <owl:Class rdf:about="http://purl.obolibrary.org/obo/GAZ_00052090">
        <rdfs:subClassOf rdf:resource="http://purl.obolibrary.org/obo/GAZ_00003034"/>
    </owl:Class>
    


    <!-- http://purl.obolibrary.org/obo/GAZ_00239919 -->

    <owl:Class rdf:about="http://purl.obolibrary.org/obo/GAZ_00239919"/>
    


    <!-- http://purl.obolibrary.org/obo/GAZ_00239929 -->

    <owl:Class rdf:about="http://purl.obolibrary.org/obo/GAZ_00239929">
        <rdfs:subClassOf rdf:resource="http://purl.obolibrary.org/obo/GAZ_00239919"/>
        <obo:IAO_0000115>A reservoir.</obo:IAO_0000115>
        <oboInOwl:hasOBONamespace>GAZ</oboInOwl:hasOBONamespace>
        <oboInOwl:id>GAZ:00239929</oboInOwl:id>
        <rdfs:label>Boskop Dam Reservoir</rdfs:label>
    </owl:Class>
    


    <!-- http://purl.obolibrary.org/obo/GAZ_00281455 -->

    <owl:Class rdf:about="http://purl.obolibrary.org/obo/GAZ_00281455"/>
    


    <!-- http://purl.obolibrary.org/obo/GAZ_00281456 -->

    <owl:Class rdf:about="http://purl.obolibrary.org/obo/GAZ_00281456">
        <rdfs:subClassOf rdf:resource="http://purl.obolibrary.org/obo/GAZ_00281455"/>
        <obo:IAO_0000115>An archeological site.</obo:IAO_0000115>
        <oboInOwl:hasOBONamespace>GAZ</oboInOwl:hasOBONamespace>
        <oboInOwl:id>GAZ:00281456</oboInOwl:id>
        <rdfs:label>Blaauboschkraal stone ruins</rdfs:label>
    </owl:Class>
    


    <!-- http://purl.obolibrary.org/obo/GAZ_00281473 -->

    <owl:Class rdf:about="http://purl.obolibrary.org/obo/GAZ_00281473"/>
    


    <!-- http://purl.obolibrary.org/obo/GAZ_00281474 -->

    <owl:Class rdf:about="http://purl.obolibrary.org/obo/GAZ_00281474">
        <rdfs:subClassOf rdf:resource="http://purl.obolibrary.org/obo/GAZ_00281473"/>
        <obo:IAO_0000115>An archeological site. A group of pre-historic stone huts; the terrain contains remainings of a settlement from the early Sotho.</obo:IAO_0000115>
        <oboInOwl:hasOBONamespace>GAZ</oboInOwl:hasOBONamespace>
        <oboInOwl:id>GAZ:00281474</oboInOwl:id>
        <rdfs:label>Sedan Beehive stone huts</rdfs:label>
    </owl:Class>
    


    <!-- http://purl.obolibrary.org/obo/GAZ_22223611 -->

    <owl:Class rdf:about="http://purl.obolibrary.org/obo/GAZ_22223611">
        <rdfs:subClassOf rdf:resource="http://purl.obolibrary.org/obo/GAZ_00003034"/>
    </owl:Class>
    


    <!-- http://purl.obolibrary.org/obo/GAZ_22223612 -->

    <owl:Class rdf:about="http://purl.obolibrary.org/obo/GAZ_22223612">
        <rdfs:subClassOf rdf:resource="http://purl.obolibrary.org/obo/GAZ_00003034"/>
    </owl:Class>
    


    <!-- http://purl.obolibrary.org/obo/GAZ_22223613 -->

    <owl:Class rdf:about="http://purl.obolibrary.org/obo/GAZ_22223613">
        <rdfs:subClassOf rdf:resource="http://purl.obolibrary.org/obo/GAZ_00003034"/>
    </owl:Class>
    


    <!-- http://purl.obolibrary.org/obo/GAZ_22223614 -->

    <owl:Class rdf:about="http://purl.obolibrary.org/obo/GAZ_22223614">
        <rdfs:subClassOf rdf:resource="http://purl.obolibrary.org/obo/GAZ_00003034"/>
    </owl:Class>
    


    <!-- http://purl.obolibrary.org/obo/GAZ_22223615 -->

    <owl:Class rdf:about="http://purl.obolibrary.org/obo/GAZ_22223615">
        <rdfs:subClassOf rdf:resource="http://purl.obolibrary.org/obo/GAZ_00003034"/>
    </owl:Class>
    


    <!-- http://purl.obolibrary.org/obo/GAZ_22223616 -->

    <owl:Class rdf:about="http://purl.obolibrary.org/obo/GAZ_22223616">
        <rdfs:subClassOf rdf:resource="http://purl.obolibrary.org/obo/GAZ_00003034"/>
    </owl:Class>
    


    <!-- http://purl.obolibrary.org/obo/GAZ_22223617 -->

    <owl:Class rdf:about="http://purl.obolibrary.org/obo/GAZ_22223617">
        <rdfs:subClassOf rdf:resource="http://purl.obolibrary.org/obo/GAZ_00003034"/>
    </owl:Class>
    


    <!-- http://purl.obolibrary.org/obo/GAZ_22223618 -->

    <owl:Class rdf:about="http://purl.obolibrary.org/obo/GAZ_22223618">
        <rdfs:subClassOf rdf:resource="http://purl.obolibrary.org/obo/GAZ_00003034"/>
    </owl:Class>
    


    <!-- http://purl.obolibrary.org/obo/GAZ_22223619 -->

    <owl:Class rdf:about="http://purl.obolibrary.org/obo/GAZ_22223619">
        <rdfs:subClassOf rdf:resource="http://purl.obolibrary.org/obo/GAZ_00003034"/>
    </owl:Class>
    


    <!-- http://purl.obolibrary.org/obo/GAZ_22223620 -->

    <owl:Class rdf:about="http://purl.obolibrary.org/obo/GAZ_22223620">
        <rdfs:subClassOf rdf:resource="http://purl.obolibrary.org/obo/GAZ_00003034"/>
    </owl:Class>
    


    <!-- http://purl.obolibrary.org/obo/GAZ_22223621 -->

    <owl:Class rdf:about="http://purl.obolibrary.org/obo/GAZ_22223621">
        <rdfs:subClassOf rdf:resource="http://purl.obolibrary.org/obo/GAZ_00003034"/>
    </owl:Class>
    


    <!-- http://purl.obolibrary.org/obo/GAZ_22223622 -->

    <owl:Class rdf:about="http://purl.obolibrary.org/obo/GAZ_22223622">
        <rdfs:subClassOf rdf:resource="http://purl.obolibrary.org/obo/GAZ_00003034"/>
    </owl:Class>
    


    <!-- http://purl.obolibrary.org/obo/GAZ_22223623 -->

    <owl:Class rdf:about="http://purl.obolibrary.org/obo/GAZ_22223623">
        <rdfs:subClassOf rdf:resource="http://purl.obolibrary.org/obo/GAZ_00003034"/>
    </owl:Class>
    


    <!-- http://purl.obolibrary.org/obo/GAZ_22223624 -->

    <owl:Class rdf:about="http://purl.obolibrary.org/obo/GAZ_22223624">
        <rdfs:subClassOf rdf:resource="http://purl.obolibrary.org/obo/GAZ_00003034"/>
    </owl:Class>
    


    <!-- http://purl.obolibrary.org/obo/GAZ_22223625 -->

    <owl:Class rdf:about="http://purl.obolibrary.org/obo/GAZ_22223625">
        <rdfs:subClassOf rdf:resource="http://purl.obolibrary.org/obo/GAZ_00003034"/>
    </owl:Class>
    


    <!-- http://purl.obolibrary.org/obo/GAZ_22223626 -->

    <owl:Class rdf:about="http://purl.obolibrary.org/obo/GAZ_22223626">
        <rdfs:subClassOf rdf:resource="http://purl.obolibrary.org/obo/GAZ_00003034"/>
    </owl:Class>
    


    <!-- http://purl.obolibrary.org/obo/GAZ_22223627 -->

    <owl:Class rdf:about="http://purl.obolibrary.org/obo/GAZ_22223627">
        <rdfs:subClassOf rdf:resource="http://purl.obolibrary.org/obo/GAZ_00003034"/>
    </owl:Class>
    


    <!-- http://purl.obolibrary.org/obo/GAZ_22223628 -->

    <owl:Class rdf:about="http://purl.obolibrary.org/obo/GAZ_22223628">
        <rdfs:subClassOf rdf:resource="http://purl.obolibrary.org/obo/GAZ_00003034"/>
    </owl:Class>
    


    <!-- http://purl.obolibrary.org/obo/GAZ_22223630 -->

    <owl:Class rdf:about="http://purl.obolibrary.org/obo/GAZ_22223630">
        <rdfs:subClassOf rdf:resource="http://purl.obolibrary.org/obo/GAZ_00003034"/>
    </owl:Class>
    


    <!-- http://purl.obolibrary.org/obo/GAZ_22224455 -->

    <owl:Class rdf:about="http://purl.obolibrary.org/obo/GAZ_22224455">
        <rdfs:subClassOf rdf:resource="http://purl.obolibrary.org/obo/GAZ_00003034"/>
    </owl:Class>
    


    <!-- 
    ///////////////////////////////////////////////////////////////////////////////////////
    //
    // Individuals
    //
    ///////////////////////////////////////////////////////////////////////////////////////
     -->

    


    <!-- http://purl.obolibrary.org/obo/GAZ_00001094 -->

    <owl:NamedIndividual rdf:about="http://purl.obolibrary.org/obo/GAZ_00001094">
        <rdf:type rdf:resource="http://purl.obolibrary.org/obo/ENVO_00000009"/>
        <obo:IAO_0000115>A country located at the southern tip of Africa. It borders the Atlantic and Indian oceans and Namibia, Botswana, Zimbabwe, Mozambique, Swaziland, and Lesotho, an independent enclave surrounded by South African territory. It is divided into nine provinces which are further subdivided into 52 districts: 6 metropolitan and 46 district municipalities. The 46 district municipalities are further subdivided into 231 local municipalities. The district municipalities also contain 20 district management areas (mostly game parks) that are directly governed by the district municipalities. The six metropolitan municipalities perform the functions of both district and local municipalities.</obo:IAO_0000115>
        <oboInOwl:hasOBONamespace>GAZ</oboInOwl:hasOBONamespace>
        <oboInOwl:id>GAZ:00001094</oboInOwl:id>
        <rdfs:label>Republic of South Africa</rdfs:label>
    </owl:NamedIndividual>
    


    <!-- http://purl.obolibrary.org/obo/GAZ_00002809 -->

    <owl:NamedIndividual rdf:about="http://purl.obolibrary.org/obo/GAZ_00002809">
        <obo:RO_0001025 rdf:resource="http://purl.obolibrary.org/obo/GAZ_00032883"/>
        <obo:IAO_0000115>A national park. To the west and south of the Kruger National Park are the two South African provinces of Mpumalanga and Limpopo. In the north is Zimbabwe, and to the east is Mozambique. It is now part of the Great Limpopo Transfrontier Park, a peace park that links Kruger National Park with the Gonarezhou National Park in Zimbabwe, and with the Limpopo National Park in Mozambique.</obo:IAO_0000115>
        <oboInOwl:hasOBONamespace>GAZ</oboInOwl:hasOBONamespace>
        <oboInOwl:id>GAZ:00002809</oboInOwl:id>
        <rdfs:label>Kruger National Park</rdfs:label>
    </owl:NamedIndividual>
    


    <!-- http://purl.obolibrary.org/obo/GAZ_00002810 -->

    <owl:NamedIndividual rdf:about="http://purl.obolibrary.org/obo/GAZ_00002810">
        <obo:RO_0001025 rdf:resource="http://purl.obolibrary.org/obo/GAZ_00001094"/>
    </owl:NamedIndividual>
    


    <!-- http://purl.obolibrary.org/obo/GAZ_00002811 -->

    <owl:NamedIndividual rdf:about="http://purl.obolibrary.org/obo/GAZ_00002811"/>
    


    <!-- http://purl.obolibrary.org/obo/GAZ_00002812 -->

    <owl:NamedIndividual rdf:about="http://purl.obolibrary.org/obo/GAZ_00002812"/>
    


    <!-- http://purl.obolibrary.org/obo/GAZ_00002813 -->

    <owl:NamedIndividual rdf:about="http://purl.obolibrary.org/obo/GAZ_00002813"/>
    


    <!-- http://purl.obolibrary.org/obo/GAZ_00002814 -->

    <owl:NamedIndividual rdf:about="http://purl.obolibrary.org/obo/GAZ_00002814"/>
    


    <!-- http://purl.obolibrary.org/obo/GAZ_00002815 -->

    <owl:NamedIndividual rdf:about="http://purl.obolibrary.org/obo/GAZ_00002815"/>
    


    <!-- http://purl.obolibrary.org/obo/GAZ_00002816 -->

    <owl:NamedIndividual rdf:about="http://purl.obolibrary.org/obo/GAZ_00002816"/>
    


    <!-- http://purl.obolibrary.org/obo/GAZ_00002817 -->

    <owl:NamedIndividual rdf:about="http://purl.obolibrary.org/obo/GAZ_00002817"/>
    


    <!-- http://purl.obolibrary.org/obo/GAZ_00002818 -->

    <owl:NamedIndividual rdf:about="http://purl.obolibrary.org/obo/GAZ_00002818"/>
    


    <!-- http://purl.obolibrary.org/obo/GAZ_00002819 -->

    <owl:NamedIndividual rdf:about="http://purl.obolibrary.org/obo/GAZ_00002819"/>
    


    <!-- http://purl.obolibrary.org/obo/GAZ_00003034 -->

    <owl:NamedIndividual rdf:about="http://purl.obolibrary.org/obo/GAZ_00003034">
        <obo:RO_0001025 rdf:resource="http://purl.obolibrary.org/obo/GAZ_00001094"/>
    </owl:NamedIndividual>
    


    <!-- http://purl.obolibrary.org/obo/GAZ_00003035 -->

    <owl:NamedIndividual rdf:about="http://purl.obolibrary.org/obo/GAZ_00003035">
        <obo:RO_0001025 rdf:resource="http://purl.obolibrary.org/obo/GAZ_00005318"/>
    </owl:NamedIndividual>
    


    <!-- http://purl.obolibrary.org/obo/GAZ_00003036 -->

    <owl:NamedIndividual rdf:about="http://purl.obolibrary.org/obo/GAZ_00003036">
        <obo:RO_0001025 rdf:resource="http://purl.obolibrary.org/obo/GAZ_00387339"/>
        <obo:IAO_0000115>A central suburb of Johannesburg, in South Africa.</obo:IAO_0000115>
        <oboInOwl:hasOBONamespace>GAZ</oboInOwl:hasOBONamespace>
        <oboInOwl:id>GAZ:00003036</oboInOwl:id>
        <rdfs:label>Braamfontein</rdfs:label>
    </owl:NamedIndividual>
    


    <!-- http://purl.obolibrary.org/obo/GAZ_00003725 -->

    <owl:NamedIndividual rdf:about="http://purl.obolibrary.org/obo/GAZ_00003725">
        <rdf:type rdf:resource="http://purl.obolibrary.org/obo/ENVO_00000856"/>
        <obo:RO_0001025 rdf:resource="http://purl.obolibrary.org/obo/GAZ_00002816"/>
    </owl:NamedIndividual>
    


    <!-- http://purl.obolibrary.org/obo/GAZ_00003726 -->

    <owl:NamedIndividual rdf:about="http://purl.obolibrary.org/obo/GAZ_00003726">
        <obo:RO_0001025 rdf:resource="http://purl.obolibrary.org/obo/GAZ_00012787"/>
    </owl:NamedIndividual>
    


    <!-- http://purl.obolibrary.org/obo/GAZ_00005305 -->

    <owl:NamedIndividual rdf:about="http://purl.obolibrary.org/obo/GAZ_00005305">
        <rdf:type rdf:resource="http://purl.obolibrary.org/obo/ENVO_00000856"/>
        <obo:RO_0001025 rdf:resource="http://purl.obolibrary.org/obo/GAZ_00012793"/>
    </owl:NamedIndividual>
    


    <!-- http://purl.obolibrary.org/obo/GAZ_00005306 -->

    <owl:NamedIndividual rdf:about="http://purl.obolibrary.org/obo/GAZ_00005306">
        <obo:RO_0001025 rdf:resource="http://purl.obolibrary.org/obo/GAZ_00009437"/>
    </owl:NamedIndividual>
    


    <!-- http://purl.obolibrary.org/obo/GAZ_00005307 -->

    <owl:NamedIndividual rdf:about="http://purl.obolibrary.org/obo/GAZ_00005307">
        <obo:RO_0001025 rdf:resource="http://purl.obolibrary.org/obo/GAZ_00076057"/>
        <obo:IAO_0000115>A city of situated in northeastern South Africa. It is the capital of the Mpumalanga province (formerly Eastern Transvaal).</obo:IAO_0000115>
        <oboInOwl:hasOBONamespace>GAZ</oboInOwl:hasOBONamespace>
        <oboInOwl:id>GAZ:00005307</oboInOwl:id>
        <rdfs:label>Mbombela</rdfs:label>
    </owl:NamedIndividual>
    


    <!-- http://purl.obolibrary.org/obo/GAZ_00005308 -->

    <owl:NamedIndividual rdf:about="http://purl.obolibrary.org/obo/GAZ_00005308">
        <obo:RO_0001025 rdf:resource="http://purl.obolibrary.org/obo/GAZ_00002812"/>
        <obo:IAO_0000115>A national park located on the east coast of KwaZulu-Natal, South Africa about 275 km north of Durban. It spans 280 km of coastline, from the Mozambican border in the north to Mapelane south of the Saint Lucia estuary. A World Heritage Site. A Ramsar Site.</obo:IAO_0000115>
        <oboInOwl:hasOBONamespace>GAZ</oboInOwl:hasOBONamespace>
        <oboInOwl:id>GAZ:00005308</oboInOwl:id>
        <rdfs:label>iSimangaliso Wetland Park</rdfs:label>
    </owl:NamedIndividual>
    


    <!-- http://purl.obolibrary.org/obo/GAZ_00005309 -->

    <owl:NamedIndividual rdf:about="http://purl.obolibrary.org/obo/GAZ_00005309">
        <obo:RO_0001025 rdf:resource="http://purl.obolibrary.org/obo/GAZ_00002812"/>
        <oboInOwl:hasOBONamespace>GAZ</oboInOwl:hasOBONamespace>
        <oboInOwl:id>GAZ:00005309</oboInOwl:id>
        <rdfs:label>Dukuduku Forest</rdfs:label>
    </owl:NamedIndividual>
    


    <!-- http://purl.obolibrary.org/obo/GAZ_00005310 -->

    <owl:NamedIndividual rdf:about="http://purl.obolibrary.org/obo/GAZ_00005310">
        <obo:RO_0001025 rdf:resource="http://purl.obolibrary.org/obo/GAZ_00032866"/>
    </owl:NamedIndividual>
    


    <!-- http://purl.obolibrary.org/obo/GAZ_00005311 -->

    <owl:NamedIndividual rdf:about="http://purl.obolibrary.org/obo/GAZ_00005311">
        <obo:RO_0001025 rdf:resource="http://purl.obolibrary.org/obo/GAZ_00009436"/>
    </owl:NamedIndividual>
    


    <!-- http://purl.obolibrary.org/obo/GAZ_00005312 -->

    <owl:NamedIndividual rdf:about="http://purl.obolibrary.org/obo/GAZ_00005312">
        <obo:RO_0001025 rdf:resource="http://purl.obolibrary.org/obo/GAZ_00002816"/>
        <oboInOwl:hasOBONamespace>GAZ</oboInOwl:hasOBONamespace>
        <oboInOwl:id>GAZ:00005312</oboInOwl:id>
        <rdfs:label>Sabie River</rdfs:label>
    </owl:NamedIndividual>
    


    <!-- http://purl.obolibrary.org/obo/GAZ_00005313 -->

    <owl:NamedIndividual rdf:about="http://purl.obolibrary.org/obo/GAZ_00005313">
        <obo:RO_0001025 rdf:resource="http://purl.obolibrary.org/obo/GAZ_00005308"/>
        <obo:RO_0001025 rdf:resource="http://purl.obolibrary.org/obo/GAZ_00075932"/>
        <obo:IAO_0000115>A freshwater endorheic polymictic lake located in the Maputaland, or Umhlabuyalingana, area of KwaZulu-Natal, on the east coast of South Africa.</obo:IAO_0000115>
        <oboInOwl:hasOBONamespace>GAZ</oboInOwl:hasOBONamespace>
        <oboInOwl:id>GAZ:00005313</oboInOwl:id>
        <rdfs:label>Lake Sibhayi</rdfs:label>
    </owl:NamedIndividual>
    


    <!-- http://purl.obolibrary.org/obo/GAZ_00005314 -->

    <owl:NamedIndividual rdf:about="http://purl.obolibrary.org/obo/GAZ_00005314">
        <rdf:type rdf:resource="http://purl.obolibrary.org/obo/ENVO_00000856"/>
        <obo:RO_0001025 rdf:resource="http://purl.obolibrary.org/obo/GAZ_00012791"/>
    </owl:NamedIndividual>
    


    <!-- http://purl.obolibrary.org/obo/GAZ_00005316 -->

    <owl:NamedIndividual rdf:about="http://purl.obolibrary.org/obo/GAZ_00005316">
        <obo:RO_0001025 rdf:resource="http://purl.obolibrary.org/obo/GAZ_00076035"/>
    </owl:NamedIndividual>
    


    <!-- http://purl.obolibrary.org/obo/GAZ_00005317 -->

    <owl:NamedIndividual rdf:about="http://purl.obolibrary.org/obo/GAZ_00005317">
        <obo:RO_0001025 rdf:resource="http://purl.obolibrary.org/obo/GAZ_00012789"/>
        <obo:IAO_0000115>A populated place. A town situated on the banks of the Mooirivier 120 km west-southwest of Johannesburg in the North West Province of South Africa.</obo:IAO_0000115>
        <oboInOwl:hasOBONamespace>GAZ</oboInOwl:hasOBONamespace>
        <oboInOwl:id>GAZ:00005317</oboInOwl:id>
        <rdfs:label>Potchefstroom</rdfs:label>
    </owl:NamedIndividual>
    


    <!-- http://purl.obolibrary.org/obo/GAZ_00005318 -->

    <owl:NamedIndividual rdf:about="http://purl.obolibrary.org/obo/GAZ_00005318">
        <obo:RO_0001025 rdf:resource="http://purl.obolibrary.org/obo/GAZ_00002815"/>
        <obo:IAO_0000115>A Metropolitan Municipality that manages and governs the city of Johannesburg, South Africa.</obo:IAO_0000115>
        <oboInOwl:hasOBONamespace>GAZ</oboInOwl:hasOBONamespace>
        <oboInOwl:id>GAZ:00005318</oboInOwl:id>
        <rdfs:label>Metropolitan Municipality of the City of Johannesburg</rdfs:label>
    </owl:NamedIndividual>
    


    <!-- http://purl.obolibrary.org/obo/GAZ_00005320 -->

    <owl:NamedIndividual rdf:about="http://purl.obolibrary.org/obo/GAZ_00005320">
        <oboInOwl:hasOBONamespace>GAZ</oboInOwl:hasOBONamespace>
        <oboInOwl:id>GAZ:00005320</oboInOwl:id>
        <rdfs:label>Swadini River</rdfs:label>
    </owl:NamedIndividual>
    


    <!-- http://purl.obolibrary.org/obo/GAZ_00008040 -->

    <owl:NamedIndividual rdf:about="http://purl.obolibrary.org/obo/GAZ_00008040">
        <obo:RO_0001025 rdf:resource="http://purl.obolibrary.org/obo/GAZ_00002812"/>
        <obo:IAO_0000115>One of the 11 districts of KwaZulu-Natal province of South Africa.</obo:IAO_0000115>
        <oboInOwl:hasOBONamespace>GAZ</oboInOwl:hasOBONamespace>
        <oboInOwl:id>GAZ:00008040</oboInOwl:id>
        <rdfs:label>Umgungundlovu District Municipality</rdfs:label>
    </owl:NamedIndividual>
    


    <!-- http://purl.obolibrary.org/obo/GAZ_00008041 -->

    <owl:NamedIndividual rdf:about="http://purl.obolibrary.org/obo/GAZ_00008041">
        <obo:RO_0001025 rdf:resource="http://purl.obolibrary.org/obo/GAZ_00075928"/>
    </owl:NamedIndividual>
    


    <!-- http://purl.obolibrary.org/obo/GAZ_00009436 -->

    <owl:NamedIndividual rdf:about="http://purl.obolibrary.org/obo/GAZ_00009436">
        <obo:RO_0001025 rdf:resource="http://purl.obolibrary.org/obo/GAZ_00002815"/>
        <obo:IAO_0000115>A metropolitan municipality contained in the province of Gauteng, South Africa, that includes the city of Pretoria.</obo:IAO_0000115>
        <oboInOwl:hasOBONamespace>GAZ</oboInOwl:hasOBONamespace>
        <oboInOwl:id>GAZ:00009436</oboInOwl:id>
        <rdfs:label>Metropolitan Municipality of the City of Tshwane</rdfs:label>
    </owl:NamedIndividual>
    


    <!-- http://purl.obolibrary.org/obo/GAZ_00009437 -->

    <owl:NamedIndividual rdf:about="http://purl.obolibrary.org/obo/GAZ_00009437">
        <obo:RO_0001025 rdf:resource="http://purl.obolibrary.org/obo/GAZ_00002817"/>
        <obo:IAO_0000115>The metropolitan municipality which governs the city of Cape Town, South Africa and its suburbs and exurbs.</obo:IAO_0000115>
        <oboInOwl:hasOBONamespace>GAZ</oboInOwl:hasOBONamespace>
        <oboInOwl:id>GAZ:00009437</oboInOwl:id>
        <rdfs:label>Metropolitan Municipality of the City of Cape Town</rdfs:label>
    </owl:NamedIndividual>
    


    <!-- http://purl.obolibrary.org/obo/GAZ_00010006 -->

    <owl:NamedIndividual rdf:about="http://purl.obolibrary.org/obo/GAZ_00010006">
        <obo:RO_0001025 rdf:resource="http://purl.obolibrary.org/obo/GAZ_00002812"/>
        <obo:IAO_0000115>The Metropolitan Municipality created in 2000 that includes the city of Durban, South Africa and surrounding towns. eThekwini is one of the 11 districts of KwaZulu-Natal province of South Africa.</obo:IAO_0000115>
        <oboInOwl:hasOBONamespace>GAZ</oboInOwl:hasOBONamespace>
        <oboInOwl:id>GAZ:00010006</oboInOwl:id>
        <rdfs:label>eThekwini Metropolitan Municipality</rdfs:label>
    </owl:NamedIndividual>
    


    <!-- http://purl.obolibrary.org/obo/GAZ_00010007 -->

    <owl:NamedIndividual rdf:about="http://purl.obolibrary.org/obo/GAZ_00010007">
        <obo:RO_0001025 rdf:resource="http://purl.obolibrary.org/obo/GAZ_00010006"/>
    </owl:NamedIndividual>
    


    <!-- http://purl.obolibrary.org/obo/GAZ_00010008 -->

    <owl:NamedIndividual rdf:about="http://purl.obolibrary.org/obo/GAZ_00010008">
        <obo:RO_0001025 rdf:resource="http://purl.obolibrary.org/obo/GAZ_00032877"/>
    </owl:NamedIndividual>
    


    <!-- http://purl.obolibrary.org/obo/GAZ_00011816 -->

    <owl:NamedIndividual rdf:about="http://purl.obolibrary.org/obo/GAZ_00011816">
        <obo:RO_0001025 rdf:resource="http://purl.obolibrary.org/obo/GAZ_00002812"/>
        <obo:IAO_0000115>A river in KwaZulu-Natal, South Africa. Its mouth is at Durban, where it is largely responsible for the formation of Durban&apos;s natural harbour. The river is approximately 232 km long with a catchment area of 4,432 km2. There are 3 large dams on the Mgeni, they are the Midmar Dam, Albert Falls Dam and Inanda Dam. A noteworthy tributary is the Msunduzi River.</obo:IAO_0000115>
        <oboInOwl:hasOBONamespace>GAZ</oboInOwl:hasOBONamespace>
        <oboInOwl:id>GAZ:00011816</oboInOwl:id>
        <rdfs:label>Mngeni River</rdfs:label>
    </owl:NamedIndividual>
    


    <!-- http://purl.obolibrary.org/obo/GAZ_00012397 -->

    <owl:NamedIndividual rdf:about="http://purl.obolibrary.org/obo/GAZ_00012397">
        <obo:RO_0001025 rdf:resource="http://purl.obolibrary.org/obo/GAZ_00052064"/>
        <oboInOwl:hasOBONamespace>GAZ</oboInOwl:hasOBONamespace>
        <oboInOwl:id>GAZ:00012397</oboInOwl:id>
        <rdfs:label>East Driefontein</rdfs:label>
    </owl:NamedIndividual>
    


    <!-- http://purl.obolibrary.org/obo/GAZ_00012398 -->

    <owl:NamedIndividual rdf:about="http://purl.obolibrary.org/obo/GAZ_00012398">
        <obo:RO_0001025 rdf:resource="http://purl.obolibrary.org/obo/GAZ_00012397"/>
        <obo:IAO_0000115>A gold mine.</obo:IAO_0000115>
        <oboInOwl:hasOBONamespace>GAZ</oboInOwl:hasOBONamespace>
        <oboInOwl:id>GAZ:00012398</oboInOwl:id>
        <rdfs:label>East Driefontein mine</rdfs:label>
    </owl:NamedIndividual>
    


    <!-- http://purl.obolibrary.org/obo/GAZ_00012399 -->

    <owl:NamedIndividual rdf:about="http://purl.obolibrary.org/obo/GAZ_00012399">
        <obo:RO_0001025 rdf:resource="http://purl.obolibrary.org/obo/GAZ_00012786"/>
        <oboInOwl:hasOBONamespace>GAZ</oboInOwl:hasOBONamespace>
        <oboInOwl:id>GAZ:00012399</oboInOwl:id>
        <rdfs:label>Carletonville</rdfs:label>
    </owl:NamedIndividual>
    


    <!-- http://purl.obolibrary.org/obo/GAZ_00012785 -->

    <owl:NamedIndividual rdf:about="http://purl.obolibrary.org/obo/GAZ_00012785">
        <obo:RO_0001025 rdf:resource="http://purl.obolibrary.org/obo/GAZ_00002815"/>
        <obo:IAO_0000115>One of the districts of Gauteng province of South Africa. The seat of West Rand is Randfontein. The urban western part of the Witwatersrand that is functionally merged with the Johannesburg conurbation.</obo:IAO_0000115>
        <oboInOwl:hasOBONamespace>GAZ</oboInOwl:hasOBONamespace>
        <oboInOwl:id>GAZ:00012785</oboInOwl:id>
        <rdfs:label>West Rand District Municipality</rdfs:label>
    </owl:NamedIndividual>
    


    <!-- http://purl.obolibrary.org/obo/GAZ_00012786 -->

    <owl:NamedIndividual rdf:about="http://purl.obolibrary.org/obo/GAZ_00012786">
        <obo:RO_0001025 rdf:resource="http://purl.obolibrary.org/obo/GAZ_00012785"/>
        <obo:IAO_0000115>A local municipality in West Rand District Municipality, Gauteng, in South Africa.</obo:IAO_0000115>
        <oboInOwl:hasOBONamespace>GAZ</oboInOwl:hasOBONamespace>
        <oboInOwl:id>GAZ:00012786</oboInOwl:id>
        <rdfs:label>Municipality of Merafong City</rdfs:label>
    </owl:NamedIndividual>
    


    <!-- http://purl.obolibrary.org/obo/GAZ_00012787 -->

    <owl:NamedIndividual rdf:about="http://purl.obolibrary.org/obo/GAZ_00012787">
        <obo:RO_0001025 rdf:resource="http://purl.obolibrary.org/obo/GAZ_00002812"/>
        <obo:IAO_0000115>One of the 11 districts of KwaZulu-Natal province of South Africa. The seat of Sisonke is Ixopo.</obo:IAO_0000115>
        <oboInOwl:hasOBONamespace>GAZ</oboInOwl:hasOBONamespace>
        <oboInOwl:id>GAZ:00012787</oboInOwl:id>
        <rdfs:label>Sisonke District Municipality</rdfs:label>
    </owl:NamedIndividual>
    


    <!-- http://purl.obolibrary.org/obo/GAZ_00012788 -->

    <owl:NamedIndividual rdf:about="http://purl.obolibrary.org/obo/GAZ_00012788">
        <obo:RO_0001025 rdf:resource="http://purl.obolibrary.org/obo/GAZ_00002814"/>
        <obo:IAO_0000115>One of the 6 districts of Limpopo province of South Africa. The seat of Sekhukhune is Groblersdal.</obo:IAO_0000115>
        <oboInOwl:hasOBONamespace>GAZ</oboInOwl:hasOBONamespace>
        <oboInOwl:id>GAZ:00012788</oboInOwl:id>
        <rdfs:label>Sekhukhune District Municipality</rdfs:label>
    </owl:NamedIndividual>
    


    <!-- http://purl.obolibrary.org/obo/GAZ_00012789 -->

    <owl:NamedIndividual rdf:about="http://purl.obolibrary.org/obo/GAZ_00012789">
        <obo:RO_0001025 rdf:resource="http://purl.obolibrary.org/obo/GAZ_00032875"/>
        <obo:IAO_0000115>A local municipality in Southern District Municipality, North West, South Africa.</obo:IAO_0000115>
        <oboInOwl:hasOBONamespace>GAZ</oboInOwl:hasOBONamespace>
        <oboInOwl:id>GAZ:00012789</oboInOwl:id>
        <rdfs:label>Potchefstroom Local Municipality</rdfs:label>
    </owl:NamedIndividual>
    


    <!-- http://purl.obolibrary.org/obo/GAZ_00012790 -->

    <owl:NamedIndividual rdf:about="http://purl.obolibrary.org/obo/GAZ_00012790">
        <obo:RO_0001025 rdf:resource="http://purl.obolibrary.org/obo/GAZ_00002817"/>
        <obo:IAO_0000115>A district municipality located in the Western Cape Province of South Africa.</obo:IAO_0000115>
        <oboInOwl:hasOBONamespace>GAZ</oboInOwl:hasOBONamespace>
        <oboInOwl:id>GAZ:00012790</oboInOwl:id>
        <rdfs:label>Cape Winelands District Municipality</rdfs:label>
    </owl:NamedIndividual>
    


    <!-- http://purl.obolibrary.org/obo/GAZ_00012791 -->

    <owl:NamedIndividual rdf:about="http://purl.obolibrary.org/obo/GAZ_00012791">
        <obo:RO_0001025 rdf:resource="http://purl.obolibrary.org/obo/GAZ_00012790"/>
        <obo:IAO_0000115>A local municipality located in the Western Cape Province of South Africa.</obo:IAO_0000115>
        <oboInOwl:hasOBONamespace>GAZ</oboInOwl:hasOBONamespace>
        <oboInOwl:id>GAZ:00012791</oboInOwl:id>
        <rdfs:label>Stellenbosch Local Municipality</rdfs:label>
    </owl:NamedIndividual>
    


    <!-- http://purl.obolibrary.org/obo/GAZ_00012792 -->

    <owl:NamedIndividual rdf:about="http://purl.obolibrary.org/obo/GAZ_00012792">
        <obo:RO_0001025 rdf:resource="http://purl.obolibrary.org/obo/GAZ_00002817"/>
        <oboInOwl:hasOBONamespace>GAZ</oboInOwl:hasOBONamespace>
        <oboInOwl:id>GAZ:00012792</oboInOwl:id>
        <rdfs:label>Eden District Municipality</rdfs:label>
    </owl:NamedIndividual>
    


    <!-- http://purl.obolibrary.org/obo/GAZ_00012793 -->

    <owl:NamedIndividual rdf:about="http://purl.obolibrary.org/obo/GAZ_00012793">
        <obo:RO_0001025 rdf:resource="http://purl.obolibrary.org/obo/GAZ_00012792"/>
        <obo:IAO_0000115>A local municipality located in the Western Cape Province of South Africa.</obo:IAO_0000115>
        <oboInOwl:hasOBONamespace>GAZ</oboInOwl:hasOBONamespace>
        <oboInOwl:id>GAZ:00012793</oboInOwl:id>
        <rdfs:label>Knysna Local Municipality</rdfs:label>
    </owl:NamedIndividual>
    


    <!-- http://purl.obolibrary.org/obo/GAZ_00014116 -->

    <owl:NamedIndividual rdf:about="http://purl.obolibrary.org/obo/GAZ_00014116">
        <obo:RO_0001025 rdf:resource="http://purl.obolibrary.org/obo/GAZ_00002817"/>
        <obo:IAO_0000115>Two small volcanic islands in the sub-antarctic Indian Ocean that are politically part of South Africa.</obo:IAO_0000115>
        <oboInOwl:hasOBONamespace>GAZ</oboInOwl:hasOBONamespace>
        <oboInOwl:id>GAZ:00014116</oboInOwl:id>
        <rdfs:label>Prince Edward Islands</rdfs:label>
    </owl:NamedIndividual>
    


    <!-- http://purl.obolibrary.org/obo/GAZ_00014117 -->

    <owl:NamedIndividual rdf:about="http://purl.obolibrary.org/obo/GAZ_00014117">
        <obo:RO_0001025 rdf:resource="http://purl.obolibrary.org/obo/GAZ_00014116"/>
        <obo:IAO_0000115>An island that lies at the SW end of a submarine plateau immediately south of the SW Indian Ocean Ridge, opposite Prince Edward Island. The low profile of 24 km wide dominantly basaltic and trachybasaltic Marion Island is formed by two young shield volcanoes that rise above a flat-topped submarine platform. The 1230 m high island is dotted by about 150 cinder cones, smaller scoria cones, and coastal tuff cones.</obo:IAO_0000115>
        <oboInOwl:hasOBONamespace>GAZ</oboInOwl:hasOBONamespace>
        <oboInOwl:id>GAZ:00014117</oboInOwl:id>
        <rdfs:label>Marion Island</rdfs:label>
    </owl:NamedIndividual>
    


    <!-- http://purl.obolibrary.org/obo/GAZ_00014118 -->

    <owl:NamedIndividual rdf:about="http://purl.obolibrary.org/obo/GAZ_00014118">
        <obo:RO_0001025 rdf:resource="http://purl.obolibrary.org/obo/GAZ_00014116"/>
        <obo:IAO_0000115>A remnant of a large shield volcano formerly centered off the current NW shore of the island. Pleistocene and Holocene scoria cones and tuff cones are located throughout the unglaciated 672 m high island, which was active contemporaneously with nearby Marion Island. Fifteen of the scoria cones and four tuff cones on the coastal plain were active during the Holocene.</obo:IAO_0000115>
        <oboInOwl:hasOBONamespace>GAZ</oboInOwl:hasOBONamespace>
        <oboInOwl:id>GAZ:00014118</oboInOwl:id>
        <rdfs:label>Prince Edward Island</rdfs:label>
    </owl:NamedIndividual>
    


    <!-- http://purl.obolibrary.org/obo/GAZ_00030269 -->

    <owl:NamedIndividual rdf:about="http://purl.obolibrary.org/obo/GAZ_00030269">
        <obo:IAO_0000115>An extensive national park in the Kalahari desert of Botswana. Also a subdistrict of Ghanzi District. Established 1961.</obo:IAO_0000115>
        <oboInOwl:hasOBONamespace>GAZ</oboInOwl:hasOBONamespace>
        <oboInOwl:id>GAZ:00030269</oboInOwl:id>
        <rdfs:label>Central Kalahari Game Reserve</rdfs:label>
    </owl:NamedIndividual>
    


    <!-- http://purl.obolibrary.org/obo/GAZ_00032845 -->

    <owl:NamedIndividual rdf:about="http://purl.obolibrary.org/obo/GAZ_00032845">
        <obo:RO_0001025 rdf:resource="http://purl.obolibrary.org/obo/GAZ_00002817"/>
        <obo:IAO_0000115>A district municipality located in the Western Cape Province of South Africa.</obo:IAO_0000115>
        <oboInOwl:hasOBONamespace>GAZ</oboInOwl:hasOBONamespace>
        <oboInOwl:id>GAZ:00032845</oboInOwl:id>
        <rdfs:label>Overberg District Municipality</rdfs:label>
    </owl:NamedIndividual>
    


    <!-- http://purl.obolibrary.org/obo/GAZ_00032855 -->

    <owl:NamedIndividual rdf:about="http://purl.obolibrary.org/obo/GAZ_00032855">
        <obo:RO_0001025 rdf:resource="http://purl.obolibrary.org/obo/GAZ_00002817"/>
        <obo:IAO_0000115>A district municipality located in the Western Cape Province of South Africa.</obo:IAO_0000115>
        <oboInOwl:hasOBONamespace>GAZ</oboInOwl:hasOBONamespace>
        <oboInOwl:id>GAZ:00032855</oboInOwl:id>
        <rdfs:label>Central Karoo District Municipality</rdfs:label>
    </owl:NamedIndividual>
    


    <!-- http://purl.obolibrary.org/obo/GAZ_00032856 -->

    <owl:NamedIndividual rdf:about="http://purl.obolibrary.org/obo/GAZ_00032856">
        <obo:RO_0001025 rdf:resource="http://purl.obolibrary.org/obo/GAZ_00002817"/>
        <obo:IAO_0000115>A district municipality located in the Western Cape Province of South Africa.</obo:IAO_0000115>
        <oboInOwl:hasOBONamespace>GAZ</oboInOwl:hasOBONamespace>
        <oboInOwl:id>GAZ:00032856</oboInOwl:id>
        <rdfs:label>West Coast District Municipality</rdfs:label>
    </owl:NamedIndividual>
    


    <!-- http://purl.obolibrary.org/obo/GAZ_00032857 -->

    <owl:NamedIndividual rdf:about="http://purl.obolibrary.org/obo/GAZ_00032857">
        <obo:RO_0001025 rdf:resource="http://purl.obolibrary.org/obo/GAZ_00002819"/>
        <obo:IAO_0000115>One of the 7 districts of Eastern Cape province of South Africa. The seat of Chris Hani is Queenstown.</obo:IAO_0000115>
        <oboInOwl:hasOBONamespace>GAZ</oboInOwl:hasOBONamespace>
        <oboInOwl:id>GAZ:00032857</oboInOwl:id>
        <rdfs:label>Chris Hani District Municipality</rdfs:label>
    </owl:NamedIndividual>
    


    <!-- http://purl.obolibrary.org/obo/GAZ_00032858 -->

    <owl:NamedIndividual rdf:about="http://purl.obolibrary.org/obo/GAZ_00032858">
        <obo:RO_0001025 rdf:resource="http://purl.obolibrary.org/obo/GAZ_00002819"/>
        <obo:IAO_0000115>A district municipality situated in the Western Portion of the Eastern Cape province.</obo:IAO_0000115>
        <oboInOwl:hasOBONamespace>GAZ</oboInOwl:hasOBONamespace>
        <oboInOwl:id>GAZ:00032858</oboInOwl:id>
        <rdfs:label>Cacadu District Municipality</rdfs:label>
    </owl:NamedIndividual>
    


    <!-- http://purl.obolibrary.org/obo/GAZ_00032859 -->

    <owl:NamedIndividual rdf:about="http://purl.obolibrary.org/obo/GAZ_00032859">
        <obo:RO_0001025 rdf:resource="http://purl.obolibrary.org/obo/GAZ_00002819"/>
        <obo:IAO_0000115>One of six Metropolitan (or Category A) municipalities in South Africa. It is located on the shores of Algoa Bay in the Eastern Cape province, and comprises the city of Port Elizabeth, the nearby towns of Uitenhage and Despatch, and the surrounding rural area.</obo:IAO_0000115>
        <oboInOwl:hasOBONamespace>GAZ</oboInOwl:hasOBONamespace>
        <oboInOwl:id>GAZ:00032859</oboInOwl:id>
        <rdfs:label>Metropolitan Municipality of Nelson Mandela</rdfs:label>
    </owl:NamedIndividual>
    


    <!-- http://purl.obolibrary.org/obo/GAZ_00032860 -->

    <owl:NamedIndividual rdf:about="http://purl.obolibrary.org/obo/GAZ_00032860">
        <obo:RO_0001025 rdf:resource="http://purl.obolibrary.org/obo/GAZ_00002819"/>
        <obo:IAO_0000115>One of the 7 districts of Eastern Cape province of South Africa. The seat of OR Tambo is Umtata.</obo:IAO_0000115>
        <oboInOwl:hasOBONamespace>GAZ</oboInOwl:hasOBONamespace>
        <oboInOwl:id>GAZ:00032860</oboInOwl:id>
        <rdfs:label>OR Thambo District Municipality</rdfs:label>
    </owl:NamedIndividual>
    


    <!-- http://purl.obolibrary.org/obo/GAZ_00032861 -->

    <owl:NamedIndividual rdf:about="http://purl.obolibrary.org/obo/GAZ_00032861">
        <obo:RO_0001025 rdf:resource="http://purl.obolibrary.org/obo/GAZ_00002819"/>
        <obo:IAO_0000115>One of the 7 districts of Eastern Cape province of South Africa. The seat of Amatole is East London.</obo:IAO_0000115>
        <oboInOwl:hasOBONamespace>GAZ</oboInOwl:hasOBONamespace>
        <oboInOwl:id>GAZ:00032861</oboInOwl:id>
        <rdfs:label>Amatole District Municipality</rdfs:label>
    </owl:NamedIndividual>
    


    <!-- http://purl.obolibrary.org/obo/GAZ_00032862 -->

    <owl:NamedIndividual rdf:about="http://purl.obolibrary.org/obo/GAZ_00032862">
        <obo:RO_0001025 rdf:resource="http://purl.obolibrary.org/obo/GAZ_00002819"/>
        <obo:IAO_0000115>One of the 7 districts of Eastern Cape province of South Africa. The seat of Ukhahlamba is Barkley East.</obo:IAO_0000115>
        <oboInOwl:hasOBONamespace>GAZ</oboInOwl:hasOBONamespace>
        <oboInOwl:id>GAZ:00032862</oboInOwl:id>
        <rdfs:label>Ukhahlamba District Municipality</rdfs:label>
    </owl:NamedIndividual>
    


    <!-- http://purl.obolibrary.org/obo/GAZ_00032863 -->

    <owl:NamedIndividual rdf:about="http://purl.obolibrary.org/obo/GAZ_00032863">
        <obo:RO_0001025 rdf:resource="http://purl.obolibrary.org/obo/GAZ_00002819"/>
        <obo:IAO_0000115>One of the 7 districts of Eastern Cape province of South Africa. The seat of Alfred Nzo is Mount Ayliff.</obo:IAO_0000115>
        <oboInOwl:hasOBONamespace>GAZ</oboInOwl:hasOBONamespace>
        <oboInOwl:id>GAZ:00032863</oboInOwl:id>
        <rdfs:label>Alfred Nzo District Municipality</rdfs:label>
    </owl:NamedIndividual>
    


    <!-- http://purl.obolibrary.org/obo/GAZ_00032864 -->

    <owl:NamedIndividual rdf:about="http://purl.obolibrary.org/obo/GAZ_00032864">
        <obo:RO_0001025 rdf:resource="http://purl.obolibrary.org/obo/GAZ_00002813"/>
        <obo:IAO_0000115>One of the 5 districts of Free State province of South Africa. The seat of Xhariep is Trompsburg.</obo:IAO_0000115>
        <oboInOwl:hasOBONamespace>GAZ</oboInOwl:hasOBONamespace>
        <oboInOwl:id>GAZ:00032864</oboInOwl:id>
        <rdfs:label>Xhariep District Municipality</rdfs:label>
    </owl:NamedIndividual>
    


    <!-- http://purl.obolibrary.org/obo/GAZ_00032865 -->

    <owl:NamedIndividual rdf:about="http://purl.obolibrary.org/obo/GAZ_00032865">
        <obo:RO_0001025 rdf:resource="http://purl.obolibrary.org/obo/GAZ_00002813"/>
        <obo:IAO_0000115>One of the 5 districts of Free State province of South Africa. The seat of Northern Free State is Sasolburg.</obo:IAO_0000115>
        <oboInOwl:hasOBONamespace>GAZ</oboInOwl:hasOBONamespace>
        <oboInOwl:id>GAZ:00032865</oboInOwl:id>
        <rdfs:label>Fezile Dabi District Municipality</rdfs:label>
    </owl:NamedIndividual>
    


    <!-- http://purl.obolibrary.org/obo/GAZ_00032866 -->

    <owl:NamedIndividual rdf:about="http://purl.obolibrary.org/obo/GAZ_00032866">
        <obo:RO_0001025 rdf:resource="http://purl.obolibrary.org/obo/GAZ_00002813"/>
        <obo:IAO_0000115>One of the 5 districts of the Free State province of South Africa. The seat of Thabo Mofutsanyane is Witsieshoek.</obo:IAO_0000115>
        <oboInOwl:hasOBONamespace>GAZ</oboInOwl:hasOBONamespace>
        <oboInOwl:id>GAZ:00032866</oboInOwl:id>
        <rdfs:label>Thabo Mofutsanyane District Municipality</rdfs:label>
    </owl:NamedIndividual>
    


    <!-- http://purl.obolibrary.org/obo/GAZ_00032867 -->

    <owl:NamedIndividual rdf:about="http://purl.obolibrary.org/obo/GAZ_00032867">
        <obo:RO_0001025 rdf:resource="http://purl.obolibrary.org/obo/GAZ_00002813"/>
        <obo:IAO_0000115>One of the 5 districts of Free State province of South Africa. The seat of Lejweleputswa is Welkom.</obo:IAO_0000115>
        <oboInOwl:hasOBONamespace>GAZ</oboInOwl:hasOBONamespace>
        <oboInOwl:id>GAZ:00032867</oboInOwl:id>
        <rdfs:label>Lejweleputswa District Municipality</rdfs:label>
    </owl:NamedIndividual>
    


    <!-- http://purl.obolibrary.org/obo/GAZ_00032868 -->

    <owl:NamedIndividual rdf:about="http://purl.obolibrary.org/obo/GAZ_00032868">
        <obo:RO_0001025 rdf:resource="http://purl.obolibrary.org/obo/GAZ_00002813"/>
        <obo:IAO_0000115>One of the 5 districts of Free State province of South Africa. The seat of Motheo is Bloemfontein.</obo:IAO_0000115>
        <oboInOwl:hasOBONamespace>GAZ</oboInOwl:hasOBONamespace>
        <oboInOwl:id>GAZ:00032868</oboInOwl:id>
        <rdfs:label>Motheo District Municipality</rdfs:label>
    </owl:NamedIndividual>
    


    <!-- http://purl.obolibrary.org/obo/GAZ_00032869 -->

    <owl:NamedIndividual rdf:about="http://purl.obolibrary.org/obo/GAZ_00032869">
        <obo:RO_0001025 rdf:resource="http://purl.obolibrary.org/obo/GAZ_00002818"/>
        <obo:IAO_0000115>One of the five districts of the Northern Cape province of South Africa. The seat of Kgalagadi is Kuruman.</obo:IAO_0000115>
        <oboInOwl:hasOBONamespace>GAZ</oboInOwl:hasOBONamespace>
        <oboInOwl:id>GAZ:00032869</oboInOwl:id>
        <rdfs:label>John Taola Gaetsewe District Municipality</rdfs:label>
    </owl:NamedIndividual>
    


    <!-- http://purl.obolibrary.org/obo/GAZ_00032870 -->

    <owl:NamedIndividual rdf:about="http://purl.obolibrary.org/obo/GAZ_00032870">
        <obo:RO_0001025 rdf:resource="http://purl.obolibrary.org/obo/GAZ_00002818"/>
        <obo:IAO_0000115>One of the 5 districts of Northern Cape province of South Africa. The seat of Frances Baard is Kimberley.</obo:IAO_0000115>
        <oboInOwl:hasOBONamespace>GAZ</oboInOwl:hasOBONamespace>
        <oboInOwl:id>GAZ:00032870</oboInOwl:id>
        <rdfs:label>Frances Baard District Municipality</rdfs:label>
    </owl:NamedIndividual>
    


    <!-- http://purl.obolibrary.org/obo/GAZ_00032871 -->

    <owl:NamedIndividual rdf:about="http://purl.obolibrary.org/obo/GAZ_00032871">
        <obo:RO_0001025 rdf:resource="http://purl.obolibrary.org/obo/GAZ_00002818"/>
        <oboInOwl:hasOBONamespace>GAZ</oboInOwl:hasOBONamespace>
        <oboInOwl:id>GAZ:00032871</oboInOwl:id>
        <rdfs:label>Karoo District Municipality</rdfs:label>
    </owl:NamedIndividual>
    


    <!-- http://purl.obolibrary.org/obo/GAZ_00032872 -->

    <owl:NamedIndividual rdf:about="http://purl.obolibrary.org/obo/GAZ_00032872">
        <rdf:type rdf:resource="http://purl.obolibrary.org/obo/ENVO_00000004"/>
        <obo:RO_0001025 rdf:resource="http://purl.obolibrary.org/obo/GAZ_00002818"/>
        <obo:IAO_0000115>A district in the Northern Cape province of South Africa.</obo:IAO_0000115>
        <oboInOwl:hasOBONamespace>GAZ</oboInOwl:hasOBONamespace>
        <oboInOwl:id>GAZ:00032872</oboInOwl:id>
        <rdfs:label>Namakwa District Municipality</rdfs:label>
    </owl:NamedIndividual>
    


    <!-- http://purl.obolibrary.org/obo/GAZ_00032873 -->

    <owl:NamedIndividual rdf:about="http://purl.obolibrary.org/obo/GAZ_00032873">
        <obo:RO_0001025 rdf:resource="http://purl.obolibrary.org/obo/GAZ_00002818"/>
        <obo:IAO_0000115>One of the 5 districts of the Northern Cape province of South Africa. The seat of Siyanda is Upington.</obo:IAO_0000115>
        <oboInOwl:hasOBONamespace>GAZ</oboInOwl:hasOBONamespace>
        <oboInOwl:id>GAZ:00032873</oboInOwl:id>
        <rdfs:label>Siyanda District Municipality</rdfs:label>
    </owl:NamedIndividual>
    


    <!-- http://purl.obolibrary.org/obo/GAZ_00032874 -->

    <owl:NamedIndividual rdf:about="http://purl.obolibrary.org/obo/GAZ_00032874">
        <obo:RO_0001025 rdf:resource="http://purl.obolibrary.org/obo/GAZ_00002811"/>
        <obo:IAO_0000115>One of the four districts of North West province in South Africa. Its capital is Mafikeng, which is also the capital of the province.</obo:IAO_0000115>
        <oboInOwl:hasOBONamespace>GAZ</oboInOwl:hasOBONamespace>
        <oboInOwl:id>GAZ:00032874</oboInOwl:id>
        <rdfs:label>Central District Municipality</rdfs:label>
    </owl:NamedIndividual>
    


    <!-- http://purl.obolibrary.org/obo/GAZ_00032875 -->

    <owl:NamedIndividual rdf:about="http://purl.obolibrary.org/obo/GAZ_00032875">
        <obo:RO_0001025 rdf:resource="http://purl.obolibrary.org/obo/GAZ_00002811"/>
        <obo:IAO_0000115>One of the 4 districts of North West province of South Africa. The seat of Southern is Klerksdorp.</obo:IAO_0000115>
        <oboInOwl:hasOBONamespace>GAZ</oboInOwl:hasOBONamespace>
        <oboInOwl:id>GAZ:00032875</oboInOwl:id>
        <rdfs:label>Southern District Municipality</rdfs:label>
    </owl:NamedIndividual>
    


    <!-- http://purl.obolibrary.org/obo/GAZ_00032876 -->

    <owl:NamedIndividual rdf:about="http://purl.obolibrary.org/obo/GAZ_00032876">
        <obo:RO_0001025 rdf:resource="http://purl.obolibrary.org/obo/GAZ_00002811"/>
        <obo:IAO_0000115>One of the 4 districts of North West province of South Africa. The seat of Bophirima is Vryberg.</obo:IAO_0000115>
        <oboInOwl:hasOBONamespace>GAZ</oboInOwl:hasOBONamespace>
        <oboInOwl:id>GAZ:00032876</oboInOwl:id>
        <rdfs:label>Bophirima District Municipality</rdfs:label>
    </owl:NamedIndividual>
    


    <!-- http://purl.obolibrary.org/obo/GAZ_00032877 -->

    <owl:NamedIndividual rdf:about="http://purl.obolibrary.org/obo/GAZ_00032877">
        <obo:RO_0001025 rdf:resource="http://purl.obolibrary.org/obo/GAZ_00002811"/>
        <obo:IAO_0000115>One of the 4 districts of North West province of South Africa. The seat of Bojanala Platinum is Rustenburg.</obo:IAO_0000115>
        <oboInOwl:hasOBONamespace>GAZ</oboInOwl:hasOBONamespace>
        <oboInOwl:id>GAZ:00032877</oboInOwl:id>
        <rdfs:label>Bojanala Platinum District Municipality</rdfs:label>
    </owl:NamedIndividual>
    


    <!-- http://purl.obolibrary.org/obo/GAZ_00032878 -->

    <owl:NamedIndividual rdf:about="http://purl.obolibrary.org/obo/GAZ_00032878">
        <obo:RO_0001025 rdf:resource="http://purl.obolibrary.org/obo/GAZ_00002815"/>
        <obo:IAO_0000115>A metropolitan municipality that forms the local government of the East Rand region of Gauteng, South Africa.</obo:IAO_0000115>
        <oboInOwl:hasOBONamespace>GAZ</oboInOwl:hasOBONamespace>
        <oboInOwl:id>GAZ:00032878</oboInOwl:id>
        <rdfs:label>Metropolitan Municipality of Ekhuruleni</rdfs:label>
    </owl:NamedIndividual>
    


    <!-- http://purl.obolibrary.org/obo/GAZ_00032879 -->

    <owl:NamedIndividual rdf:about="http://purl.obolibrary.org/obo/GAZ_00032879">
        <obo:RO_0001025 rdf:resource="http://purl.obolibrary.org/obo/GAZ_00002815"/>
        <obo:IAO_0000115>One of the districts of Gauteng province of South Africa. The seat of Sedibeng is Vereeniging.</obo:IAO_0000115>
        <oboInOwl:hasOBONamespace>GAZ</oboInOwl:hasOBONamespace>
        <oboInOwl:id>GAZ:00032879</oboInOwl:id>
        <rdfs:label>Sedibeng District Municipality</rdfs:label>
    </owl:NamedIndividual>
    


    <!-- http://purl.obolibrary.org/obo/GAZ_00032880 -->

    <owl:NamedIndividual rdf:about="http://purl.obolibrary.org/obo/GAZ_00032880">
        <obo:RO_0001025 rdf:resource="http://purl.obolibrary.org/obo/GAZ_00002815"/>
        <obo:IAO_0000115>One of the 6 districts of Gauteng province of South Africa. The seat of Metsweding is Bronkhorstspruit.</obo:IAO_0000115>
        <oboInOwl:hasOBONamespace>GAZ</oboInOwl:hasOBONamespace>
        <oboInOwl:id>GAZ:00032880</oboInOwl:id>
        <rdfs:label>Metsweding District Municipality</rdfs:label>
    </owl:NamedIndividual>
    


    <!-- http://purl.obolibrary.org/obo/GAZ_00032881 -->

    <owl:NamedIndividual rdf:about="http://purl.obolibrary.org/obo/GAZ_00032881">
        <obo:RO_0001025 rdf:resource="http://purl.obolibrary.org/obo/GAZ_00002814"/>
        <obo:IAO_0000115>One of the 6 districts of Limpopo province of South Africa. The seat of Waterberg is Modimolle. The municipality contains much of the Waterberg Biosphere, a UNESCO designated Biosphere Reserve.</obo:IAO_0000115>
        <oboInOwl:hasOBONamespace>GAZ</oboInOwl:hasOBONamespace>
        <oboInOwl:id>GAZ:00032881</oboInOwl:id>
        <rdfs:label>Waterberg District Municipality</rdfs:label>
    </owl:NamedIndividual>
    


    <!-- http://purl.obolibrary.org/obo/GAZ_00032882 -->

    <owl:NamedIndividual rdf:about="http://purl.obolibrary.org/obo/GAZ_00032882">
        <obo:RO_0001025 rdf:resource="http://purl.obolibrary.org/obo/GAZ_00002814"/>
        <obo:IAO_0000115>One of the 6 districts of Limpopo province of South Africa. It is the northernmost district of the country. The seat of Vhembe is Thohoyandou.</obo:IAO_0000115>
        <oboInOwl:hasOBONamespace>GAZ</oboInOwl:hasOBONamespace>
        <oboInOwl:id>GAZ:00032882</oboInOwl:id>
        <rdfs:label>Vhembe District Municipality</rdfs:label>
    </owl:NamedIndividual>
    


    <!-- http://purl.obolibrary.org/obo/GAZ_00032883 -->

    <owl:NamedIndividual rdf:about="http://purl.obolibrary.org/obo/GAZ_00032883">
        <obo:RO_0001025 rdf:resource="http://purl.obolibrary.org/obo/GAZ_00002814"/>
        <obo:IAO_0000115>One of the 6 districts of Limpopo province of South Africa. The seat of Mopani is Giyani.</obo:IAO_0000115>
        <oboInOwl:hasOBONamespace>GAZ</oboInOwl:hasOBONamespace>
        <oboInOwl:id>GAZ:00032883</oboInOwl:id>
        <rdfs:label>Mopani District Municipality</rdfs:label>
    </owl:NamedIndividual>
    


    <!-- http://purl.obolibrary.org/obo/GAZ_00032884 -->

    <owl:NamedIndividual rdf:about="http://purl.obolibrary.org/obo/GAZ_00032884">
        <obo:RO_0001025 rdf:resource="http://purl.obolibrary.org/obo/GAZ_00002814"/>
        <obo:IAO_0000115>One of the 6 districts of Limpopo province of South Africa. The seat of Capricorn is Polokwane.</obo:IAO_0000115>
        <oboInOwl:hasOBONamespace>GAZ</oboInOwl:hasOBONamespace>
        <oboInOwl:id>GAZ:00032884</oboInOwl:id>
        <rdfs:label>Capricorn District Municipality</rdfs:label>
    </owl:NamedIndividual>
    


    <!-- http://purl.obolibrary.org/obo/GAZ_00032885 -->

    <owl:NamedIndividual rdf:about="http://purl.obolibrary.org/obo/GAZ_00032885">
        <obo:RO_0001025 rdf:resource="http://purl.obolibrary.org/obo/GAZ_00002816"/>
        <obo:IAO_0000115>One of the 3 districts of Mpumalanga province of South Africa. The seat of Gert Sibande is Secunda.</obo:IAO_0000115>
        <oboInOwl:hasOBONamespace>GAZ</oboInOwl:hasOBONamespace>
        <oboInOwl:id>GAZ:00032885</oboInOwl:id>
        <rdfs:label>Gert Sibande District Municipality</rdfs:label>
    </owl:NamedIndividual>
    


    <!-- http://purl.obolibrary.org/obo/GAZ_00032886 -->

    <owl:NamedIndividual rdf:about="http://purl.obolibrary.org/obo/GAZ_00032886">
        <obo:RO_0001025 rdf:resource="http://purl.obolibrary.org/obo/GAZ_00002816"/>
        <obo:IAO_0000115>One of the 3 districts of Mpumalanga province of South Africa. The seat of Nkangala is Middelburg.</obo:IAO_0000115>
        <oboInOwl:hasOBONamespace>GAZ</oboInOwl:hasOBONamespace>
        <oboInOwl:id>GAZ:00032886</oboInOwl:id>
        <rdfs:label>Nkangala District Municipality</rdfs:label>
    </owl:NamedIndividual>
    


    <!-- http://purl.obolibrary.org/obo/GAZ_00032887 -->

    <owl:NamedIndividual rdf:about="http://purl.obolibrary.org/obo/GAZ_00032887">
        <obo:RO_0001025 rdf:resource="http://purl.obolibrary.org/obo/GAZ_00002816"/>
        <obo:IAO_0000115>One of the 3 districts of Mpumalanga province of South Africa. The seat of Ehlanzeni is Nelspruit.</obo:IAO_0000115>
        <oboInOwl:hasOBONamespace>GAZ</oboInOwl:hasOBONamespace>
        <oboInOwl:id>GAZ:00032887</oboInOwl:id>
        <rdfs:label>Ehlanzeni District Municipality</rdfs:label>
    </owl:NamedIndividual>
    


    <!-- http://purl.obolibrary.org/obo/GAZ_00032888 -->

    <owl:NamedIndividual rdf:about="http://purl.obolibrary.org/obo/GAZ_00032888">
        <obo:RO_0001025 rdf:resource="http://purl.obolibrary.org/obo/GAZ_00002812"/>
        <obo:IAO_0000115>One of the 11 district municipalities (&quot;districts&quot;) of KwaZulu-Natal province in South Africa. The seat of Umzinyathi is Dundee.</obo:IAO_0000115>
        <oboInOwl:hasOBONamespace>GAZ</oboInOwl:hasOBONamespace>
        <oboInOwl:id>GAZ:00032888</oboInOwl:id>
        <rdfs:label>Umzinyathi District Municipality</rdfs:label>
    </owl:NamedIndividual>
    


    <!-- http://purl.obolibrary.org/obo/GAZ_00032889 -->

    <owl:NamedIndividual rdf:about="http://purl.obolibrary.org/obo/GAZ_00032889">
        <obo:RO_0001025 rdf:resource="http://purl.obolibrary.org/obo/GAZ_00002812"/>
        <obo:IAO_0000115>One of the 11 districts of KwaZulu-Natal province of South Africa. The seat of Uthukela is the town of Ladysmith.</obo:IAO_0000115>
        <oboInOwl:hasOBONamespace>GAZ</oboInOwl:hasOBONamespace>
        <oboInOwl:id>GAZ:00032889</oboInOwl:id>
        <rdfs:label>Uthukela District Municipality</rdfs:label>
    </owl:NamedIndividual>
    


    <!-- http://purl.obolibrary.org/obo/GAZ_00032890 -->

    <owl:NamedIndividual rdf:about="http://purl.obolibrary.org/obo/GAZ_00032890">
        <obo:RO_0001025 rdf:resource="http://purl.obolibrary.org/obo/GAZ_00002812"/>
        <obo:IAO_0000115>One of the 11 district municipalities of KwaZulu-Natal province. The seat of Zululand is Ulundi.</obo:IAO_0000115>
        <oboInOwl:hasOBONamespace>GAZ</oboInOwl:hasOBONamespace>
        <oboInOwl:id>GAZ:00032890</oboInOwl:id>
        <rdfs:label>Zululand District Municipality</rdfs:label>
    </owl:NamedIndividual>
    


    <!-- http://purl.obolibrary.org/obo/GAZ_00032891 -->

    <owl:NamedIndividual rdf:about="http://purl.obolibrary.org/obo/GAZ_00032891">
        <obo:RO_0001025 rdf:resource="http://purl.obolibrary.org/obo/GAZ_00002812"/>
        <obo:IAO_0000115>One of the 11 districts of KwaZulu-Natal province of South Africa.</obo:IAO_0000115>
        <oboInOwl:hasOBONamespace>GAZ</oboInOwl:hasOBONamespace>
        <oboInOwl:id>GAZ:00032891</oboInOwl:id>
        <rdfs:label>uThungulu District Municipality</rdfs:label>
    </owl:NamedIndividual>
    


    <!-- http://purl.obolibrary.org/obo/GAZ_00032892 -->

    <owl:NamedIndividual rdf:about="http://purl.obolibrary.org/obo/GAZ_00032892">
        <obo:RO_0001025 rdf:resource="http://purl.obolibrary.org/obo/GAZ_00002812"/>
        <obo:IAO_0000115>One of the 11 districts of KwaZulu-Natal province. The seat of Amajuba is Newcastle.</obo:IAO_0000115>
        <oboInOwl:hasOBONamespace>GAZ</oboInOwl:hasOBONamespace>
        <oboInOwl:id>GAZ:00032892</oboInOwl:id>
        <rdfs:label>Amajuba District Municipality</rdfs:label>
    </owl:NamedIndividual>
    


    <!-- http://purl.obolibrary.org/obo/GAZ_00032893 -->

    <owl:NamedIndividual rdf:about="http://purl.obolibrary.org/obo/GAZ_00032893">
        <obo:RO_0001025 rdf:resource="http://purl.obolibrary.org/obo/GAZ_00002812"/>
        <obo:IAO_0000115>One of the 11 district municipalities (&quot;districts&quot;) of KwaZulu-Natal province in South Africa. The seat of iLembe is KwaDukuza.</obo:IAO_0000115>
        <oboInOwl:hasOBONamespace>GAZ</oboInOwl:hasOBONamespace>
        <oboInOwl:id>GAZ:00032893</oboInOwl:id>
        <rdfs:label>iLembe District Municipality</rdfs:label>
    </owl:NamedIndividual>
    


    <!-- http://purl.obolibrary.org/obo/GAZ_00032894 -->

    <owl:NamedIndividual rdf:about="http://purl.obolibrary.org/obo/GAZ_00032894">
        <obo:RO_0001025 rdf:resource="http://purl.obolibrary.org/obo/GAZ_00002812"/>
        <obo:IAO_0000115>One of the 11 districts of KwaZulu-Natal province of South Africa. The seat of Ugu is Port Shepstone.</obo:IAO_0000115>
        <oboInOwl:hasOBONamespace>GAZ</oboInOwl:hasOBONamespace>
        <oboInOwl:id>GAZ:00032894</oboInOwl:id>
        <rdfs:label>Ugu District Municipality</rdfs:label>
    </owl:NamedIndividual>
    


    <!-- http://purl.obolibrary.org/obo/GAZ_00040025 -->

    <owl:NamedIndividual rdf:about="http://purl.obolibrary.org/obo/GAZ_00040025">
        <obo:RO_0001025 rdf:resource="http://purl.obolibrary.org/obo/GAZ_00002817"/>
        <obo:IAO_0000115>An island in the Atlantic Ocean. It is situated about 10 km west of Yzerfontein and 55 km north of Cape Town. The flat and low-lying island measures about 4.5 km long by 2 km wide and is a proclaimed nature reserve.</obo:IAO_0000115>
        <oboInOwl:hasOBONamespace>GAZ</oboInOwl:hasOBONamespace>
        <oboInOwl:id>GAZ:00040025</oboInOwl:id>
        <rdfs:label>Dassen Island</rdfs:label>
    </owl:NamedIndividual>
    


    <!-- http://purl.obolibrary.org/obo/GAZ_00040026 -->

    <owl:NamedIndividual rdf:about="http://purl.obolibrary.org/obo/GAZ_00040026">
        <obo:RO_0001025 rdf:resource="http://purl.obolibrary.org/obo/GAZ_00040027"/>
        <obo:IAO_0000115>An island in Table Bay, 12 km off the coast from Cape Town, South Africa.</obo:IAO_0000115>
        <oboInOwl:hasOBONamespace>GAZ</oboInOwl:hasOBONamespace>
        <oboInOwl:id>GAZ:00040026</oboInOwl:id>
        <rdfs:label>Robben Island</rdfs:label>
    </owl:NamedIndividual>
    


    <!-- http://purl.obolibrary.org/obo/GAZ_00040027 -->

    <owl:NamedIndividual rdf:about="http://purl.obolibrary.org/obo/GAZ_00040027">
        <obo:RO_0001025 rdf:resource="http://purl.obolibrary.org/obo/GAZ_00009437"/>
        <obo:IAO_0000115>A natural inlet overlooked by Cape Town and is at the northern end of the Cape Peninsula, which stretches south to the Cape of Good Hope.</obo:IAO_0000115>
        <oboInOwl:hasOBONamespace>GAZ</oboInOwl:hasOBONamespace>
        <oboInOwl:id>GAZ:00040027</oboInOwl:id>
        <rdfs:label>Table Bay</rdfs:label>
    </owl:NamedIndividual>
    


    <!-- http://purl.obolibrary.org/obo/GAZ_00040028 -->

    <owl:NamedIndividual rdf:about="http://purl.obolibrary.org/obo/GAZ_00040028">
        <obo:RO_0001025 rdf:resource="http://purl.obolibrary.org/obo/GAZ_00009437"/>
        <obo:IAO_0000115>A body of water defined by the Cape Peninsula and Cape Hangklip to the east. Cape Point and the Cape of Good Hope are very close to each other on the other side of the bay, at the extreme southern tip of the Cape Peninsula.</obo:IAO_0000115>
        <oboInOwl:hasOBONamespace>GAZ</oboInOwl:hasOBONamespace>
        <oboInOwl:id>GAZ:00040028</oboInOwl:id>
        <rdfs:label>False Bay</rdfs:label>
    </owl:NamedIndividual>
    


    <!-- http://purl.obolibrary.org/obo/GAZ_00040029 -->

    <owl:NamedIndividual rdf:about="http://purl.obolibrary.org/obo/GAZ_00040029">
        <obo:RO_0001025 rdf:resource="http://purl.obolibrary.org/obo/GAZ_00040028"/>
        <obo:IAO_0000115>A small island located about 5.7 km off the northern beaches of False Bay, near Cape Town, in South Africa.</obo:IAO_0000115>
        <oboInOwl:hasOBONamespace>GAZ</oboInOwl:hasOBONamespace>
        <oboInOwl:id>GAZ:00040029</oboInOwl:id>
        <rdfs:label>Seal Island</rdfs:label>
    </owl:NamedIndividual>
    


    <!-- http://purl.obolibrary.org/obo/GAZ_00052064 -->

    <owl:NamedIndividual rdf:about="http://purl.obolibrary.org/obo/GAZ_00052064"/>
    


    <!-- http://purl.obolibrary.org/obo/GAZ_00052087 -->

    <owl:NamedIndividual rdf:about="http://purl.obolibrary.org/obo/GAZ_00052087">
        <obo:RO_0001025 rdf:resource="http://purl.obolibrary.org/obo/GAZ_00032859"/>
    </owl:NamedIndividual>
    


    <!-- http://purl.obolibrary.org/obo/GAZ_00052088 -->

    <owl:NamedIndividual rdf:about="http://purl.obolibrary.org/obo/GAZ_00052088">
        <obo:RO_0001025 rdf:resource="http://purl.obolibrary.org/obo/GAZ_00052087"/>
        <obo:IAO_0000115>A small lead-copper mine.</obo:IAO_0000115>
        <oboInOwl:hasOBONamespace>GAZ</oboInOwl:hasOBONamespace>
        <oboInOwl:id>GAZ:00052088</oboInOwl:id>
        <rdfs:label>Maitland Mine</rdfs:label>
    </owl:NamedIndividual>
    


    <!-- http://purl.obolibrary.org/obo/GAZ_00052089 -->

    <owl:NamedIndividual rdf:about="http://purl.obolibrary.org/obo/GAZ_00052089">
        <obo:RO_0001025 rdf:resource="http://purl.obolibrary.org/obo/GAZ_00052087"/>
        <oboInOwl:hasOBONamespace>GAZ</oboInOwl:hasOBONamespace>
        <oboInOwl:id>GAZ:00052089</oboInOwl:id>
        <rdfs:label>Maitland Mines colony</rdfs:label>
    </owl:NamedIndividual>
    


    <!-- http://purl.obolibrary.org/obo/GAZ_00052090 -->

    <owl:NamedIndividual rdf:about="http://purl.obolibrary.org/obo/GAZ_00052090">
        <obo:RO_0001025 rdf:resource="http://purl.obolibrary.org/obo/GAZ_00032867"/>
    </owl:NamedIndividual>
    


    <!-- http://purl.obolibrary.org/obo/GAZ_00052091 -->

    <owl:NamedIndividual rdf:about="http://purl.obolibrary.org/obo/GAZ_00052091">
        <obo:RO_0001025 rdf:resource="http://purl.obolibrary.org/obo/GAZ_00052090"/>
        <obo:IAO_0000115>A gold mine. 30 km north of Welkom.</obo:IAO_0000115>
        <oboInOwl:hasOBONamespace>GAZ</oboInOwl:hasOBONamespace>
        <oboInOwl:id>GAZ:00052091</oboInOwl:id>
        <rdfs:label>Target mine</rdfs:label>
    </owl:NamedIndividual>
    


    <!-- http://purl.obolibrary.org/obo/GAZ_00053778 -->

    <owl:NamedIndividual rdf:about="http://purl.obolibrary.org/obo/GAZ_00053778">
        <obo:RO_0001025 rdf:resource="http://purl.obolibrary.org/obo/GAZ_00014117"/>
        <obo:IAO_0000115>The highest mountain on Marion Island.</obo:IAO_0000115>
        <oboInOwl:hasOBONamespace>GAZ</oboInOwl:hasOBONamespace>
        <oboInOwl:id>GAZ:00053778</oboInOwl:id>
        <rdfs:label>Mascarin Peak</rdfs:label>
    </owl:NamedIndividual>
    


    <!-- http://purl.obolibrary.org/obo/GAZ_00053779 -->

    <owl:NamedIndividual rdf:about="http://purl.obolibrary.org/obo/GAZ_00053779">
        <obo:RO_0001025 rdf:resource="http://purl.obolibrary.org/obo/GAZ_00014116"/>
        <obo:IAO_0000115>A satellite rock 150 m off the northern coast of Marion Island.</obo:IAO_0000115>
        <oboInOwl:hasOBONamespace>GAZ</oboInOwl:hasOBONamespace>
        <oboInOwl:id>GAZ:00053779</oboInOwl:id>
        <rdfs:label>Boot Rock</rdfs:label>
    </owl:NamedIndividual>
    


    <!-- http://purl.obolibrary.org/obo/GAZ_00053780 -->

    <owl:NamedIndividual rdf:about="http://purl.obolibrary.org/obo/GAZ_00053780">
        <obo:RO_0001025 rdf:resource="http://purl.obolibrary.org/obo/GAZ_00014118"/>
        <obo:IAO_0000115>The highest peak of Prince Edward Island.</obo:IAO_0000115>
        <oboInOwl:hasOBONamespace>GAZ</oboInOwl:hasOBONamespace>
        <oboInOwl:id>GAZ:00053780</oboInOwl:id>
        <rdfs:label>Von Zinderen Bakker Peak</rdfs:label>
    </owl:NamedIndividual>
    


    <!-- http://purl.obolibrary.org/obo/GAZ_00053781 -->

    <owl:NamedIndividual rdf:about="http://purl.obolibrary.org/obo/GAZ_00053781">
        <obo:RO_0001025 rdf:resource="http://purl.obolibrary.org/obo/GAZ_00014116"/>
        <obo:IAO_0000115>Satellite rocks off Prince Edward Island (500 meters, 1650 ft, from the shore).</obo:IAO_0000115>
        <oboInOwl:hasOBONamespace>GAZ</oboInOwl:hasOBONamespace>
        <oboInOwl:id>GAZ:00053781</oboInOwl:id>
        <rdfs:label>Ross Rocks</rdfs:label>
    </owl:NamedIndividual>
    


    <!-- http://purl.obolibrary.org/obo/GAZ_00053782 -->

    <owl:NamedIndividual rdf:about="http://purl.obolibrary.org/obo/GAZ_00053782">
        <obo:RO_0001025 rdf:resource="http://purl.obolibrary.org/obo/GAZ_00014116"/>
        <obo:IAO_0000115>A satellite rock off Prince Edward Island (100 meters, 330 ft, north of northernmost point).</obo:IAO_0000115>
        <oboInOwl:hasOBONamespace>GAZ</oboInOwl:hasOBONamespace>
        <oboInOwl:id>GAZ:00053782</oboInOwl:id>
        <rdfs:label>Ship Rock</rdfs:label>
    </owl:NamedIndividual>
    


    <!-- http://purl.obolibrary.org/obo/GAZ_00053783 -->

    <owl:NamedIndividual rdf:about="http://purl.obolibrary.org/obo/GAZ_00053783">
        <obo:RO_0001025 rdf:resource="http://purl.obolibrary.org/obo/GAZ_00014117"/>
        <obo:IAO_0000115>A scientitific research station of the South African National Antarctic Programme.</obo:IAO_0000115>
        <oboInOwl:hasOBONamespace>GAZ</oboInOwl:hasOBONamespace>
        <oboInOwl:id>GAZ:00053783</oboInOwl:id>
        <rdfs:label>Marion Island Meteorological Station</rdfs:label>
    </owl:NamedIndividual>
    


    <!-- http://purl.obolibrary.org/obo/GAZ_00056666 -->

    <owl:NamedIndividual rdf:about="http://purl.obolibrary.org/obo/GAZ_00056666">
        <obo:RO_0001025 rdf:resource="http://purl.obolibrary.org/obo/GAZ_00001094"/>
        <obo:IAO_0000115>A mountain range in South Africa.</obo:IAO_0000115>
        <oboInOwl:hasOBONamespace>GAZ</oboInOwl:hasOBONamespace>
        <oboInOwl:id>GAZ:00056666</oboInOwl:id>
        <rdfs:label>Kelsaburke Mountains</rdfs:label>
    </owl:NamedIndividual>
    


    <!-- http://purl.obolibrary.org/obo/GAZ_00057762 -->

    <owl:NamedIndividual rdf:about="http://purl.obolibrary.org/obo/GAZ_00057762">
        <obo:RO_0001025 rdf:resource="http://purl.obolibrary.org/obo/GAZ_00002818"/>
        <obo:IAO_0000115>A mountainous desert in Northern Cape Province, Republic of South Africa. It is located in South Africa&apos;s northern Namaqualand.</obo:IAO_0000115>
        <oboInOwl:hasOBONamespace>GAZ</oboInOwl:hasOBONamespace>
        <oboInOwl:id>GAZ:00057762</oboInOwl:id>
        <rdfs:label>Richtersveld</rdfs:label>
    </owl:NamedIndividual>
    


    <!-- http://purl.obolibrary.org/obo/GAZ_00057764 -->

    <owl:NamedIndividual rdf:about="http://purl.obolibrary.org/obo/GAZ_00057764">
        <obo:IAO_0000115>The N part of Namaqualand, located in the Karas Region of Namibia.</obo:IAO_0000115>
        <oboInOwl:hasOBONamespace>GAZ</oboInOwl:hasOBONamespace>
        <oboInOwl:id>GAZ:00057764</oboInOwl:id>
        <rdfs:label>Great Namaqualand</rdfs:label>
    </owl:NamedIndividual>
    


    <!-- http://purl.obolibrary.org/obo/GAZ_00057765 -->

    <owl:NamedIndividual rdf:about="http://purl.obolibrary.org/obo/GAZ_00057765">
        <obo:RO_0001025 rdf:resource="http://purl.obolibrary.org/obo/GAZ_22223594"/>
        <obo:IAO_0000115>The S part of Namaqualand, located in Northern Cape Province, Republic of South Africa.</obo:IAO_0000115>
        <oboInOwl:hasOBONamespace>GAZ</oboInOwl:hasOBONamespace>
        <oboInOwl:id>GAZ:00057765</oboInOwl:id>
        <rdfs:label>Little Namaqualand</rdfs:label>
    </owl:NamedIndividual>
    


    <!-- http://purl.obolibrary.org/obo/GAZ_00058774 -->

    <owl:NamedIndividual rdf:about="http://purl.obolibrary.org/obo/GAZ_00058774">
        <obo:IAO_0000115>A reservoir on the Mwenezi River in southern Zimbabwe. It is located in the Mwenezi District.</obo:IAO_0000115>
        <oboInOwl:hasOBONamespace>GAZ</oboInOwl:hasOBONamespace>
        <oboInOwl:id>GAZ:00058774</oboInOwl:id>
        <rdfs:label>Lake Manyuchi</rdfs:label>
    </owl:NamedIndividual>
    


    <!-- http://purl.obolibrary.org/obo/GAZ_00058776 -->

    <owl:NamedIndividual rdf:about="http://purl.obolibrary.org/obo/GAZ_00058776">
        <obo:RO_0001025 rdf:resource="http://purl.obolibrary.org/obo/GAZ_00237631"/>
        <obo:IAO_0000115>A reservoir in south eastern Zimbabwe, SE of Masvingo. Rivers which feed the lake include the Mbebvi River, Matare River, Pokoteke River, Umpopinyani River, Makurumidzi River and Shagashe River. Impounded by the Kyle Dam. Constructed 1960.</obo:IAO_0000115>
        <oboInOwl:hasOBONamespace>GAZ</oboInOwl:hasOBONamespace>
        <oboInOwl:id>GAZ:00058776</oboInOwl:id>
        <rdfs:label>Lake Mutirikwe</rdfs:label>
    </owl:NamedIndividual>
    


    <!-- http://purl.obolibrary.org/obo/GAZ_00058814 -->

    <owl:NamedIndividual rdf:about="http://purl.obolibrary.org/obo/GAZ_00058814">
        <obo:RO_0001025 rdf:resource="http://purl.obolibrary.org/obo/GAZ_00032879"/>
        <obo:IAO_0000115>A dam, constructed in 1938, on the Vaal River.</obo:IAO_0000115>
        <oboInOwl:hasOBONamespace>GAZ</oboInOwl:hasOBONamespace>
        <oboInOwl:id>GAZ:00058814</oboInOwl:id>
        <rdfs:label>Vaal Dam</rdfs:label>
    </owl:NamedIndividual>
    


    <!-- http://purl.obolibrary.org/obo/GAZ_00058815 -->

    <owl:NamedIndividual rdf:about="http://purl.obolibrary.org/obo/GAZ_00058815">
        <obo:RO_0001025 rdf:resource="http://purl.obolibrary.org/obo/GAZ_00032879"/>
        <obo:IAO_0000115>A reservoir caused by the construction of the Vaal Dam in 1938. Three Provinces make up the coastline. The Free State is the largest by area, Mpumalanga, and Gauteng.</obo:IAO_0000115>
        <oboInOwl:hasOBONamespace>GAZ</oboInOwl:hasOBONamespace>
        <oboInOwl:id>GAZ:00058815</oboInOwl:id>
        <rdfs:label>Vaal Dam Lake</rdfs:label>
    </owl:NamedIndividual>
    


    <!-- http://purl.obolibrary.org/obo/GAZ_00058870 -->

    <owl:NamedIndividual rdf:about="http://purl.obolibrary.org/obo/GAZ_00058870">
        <obo:RO_0001025 rdf:resource="http://purl.obolibrary.org/obo/GAZ_00058871"/>
        <obo:IAO_0000115>A polymictic freshwater lake located on the Cape Flats near Cape Town in the Western Cape Province. Its outflow is by the Zeekoe Canal.</obo:IAO_0000115>
        <oboInOwl:hasOBONamespace>GAZ</oboInOwl:hasOBONamespace>
        <oboInOwl:id>GAZ:00058870</oboInOwl:id>
        <rdfs:label>Zeekoevlei</rdfs:label>
    </owl:NamedIndividual>
    


    <!-- http://purl.obolibrary.org/obo/GAZ_00058871 -->

    <owl:NamedIndividual rdf:about="http://purl.obolibrary.org/obo/GAZ_00058871">
        <obo:RO_0001025 rdf:resource="http://purl.obolibrary.org/obo/GAZ_00005306"/>
        <obo:IAO_0000115>An expansive, low-lying, flat area situated to the southeast of the central business district of Cape Town. In geological terms, the area is essentially a vast sheet of aeolian sand, ultimately of marine origin, which has blown up from the adjacent beaches over something of the order of a hundred thousand years.</obo:IAO_0000115>
        <oboInOwl:hasOBONamespace>GAZ</oboInOwl:hasOBONamespace>
        <oboInOwl:id>GAZ:00058871</oboInOwl:id>
        <rdfs:label>Cape Flats</rdfs:label>
    </owl:NamedIndividual>
    


    <!-- http://purl.obolibrary.org/obo/GAZ_00075390 -->

    <owl:NamedIndividual rdf:about="http://purl.obolibrary.org/obo/GAZ_00075390">
        <obo:IAO_0000115>A national park in Gaza Province, Mozambique. It forms part of the Great Limpopo Transfrontier Park with the Kruger National Park, South Africa and the Gonarezhou National Park, Zimbabwe.</obo:IAO_0000115>
        <oboInOwl:hasOBONamespace>GAZ</oboInOwl:hasOBONamespace>
        <oboInOwl:id>GAZ:00075390</oboInOwl:id>
        <rdfs:label>Limpopo National Park</rdfs:label>
    </owl:NamedIndividual>
    


    <!-- http://purl.obolibrary.org/obo/GAZ_00075392 -->

    <owl:NamedIndividual rdf:about="http://purl.obolibrary.org/obo/GAZ_00075392">
        <obo:IAO_0000115>A game reserve in south-eastern Zimbabwe. It is situated in a relatively remote corner of Masvingo Province, south of Chimanimani along the Mozambique border.</obo:IAO_0000115>
        <oboInOwl:hasOBONamespace>GAZ</oboInOwl:hasOBONamespace>
        <oboInOwl:id>GAZ:00075392</oboInOwl:id>
        <rdfs:label>Gonarezhou National Park</rdfs:label>
    </owl:NamedIndividual>
    


    <!-- http://purl.obolibrary.org/obo/GAZ_00075393 -->

    <owl:NamedIndividual rdf:about="http://purl.obolibrary.org/obo/GAZ_00075393">
        <oboInOwl:hasOBONamespace>GAZ</oboInOwl:hasOBONamespace>
        <oboInOwl:id>GAZ:00075393</oboInOwl:id>
        <rdfs:label>Malipati Safari Area</rdfs:label>
    </owl:NamedIndividual>
    


    <!-- http://purl.obolibrary.org/obo/GAZ_00075394 -->

    <owl:NamedIndividual rdf:about="http://purl.obolibrary.org/obo/GAZ_00075394">
        <oboInOwl:hasOBONamespace>GAZ</oboInOwl:hasOBONamespace>
        <oboInOwl:id>GAZ:00075394</oboInOwl:id>
        <rdfs:label>Manjinji Pan Sanctuary</rdfs:label>
    </owl:NamedIndividual>
    


    <!-- http://purl.obolibrary.org/obo/GAZ_00075413 -->

    <owl:NamedIndividual rdf:about="http://purl.obolibrary.org/obo/GAZ_00075413">
        <obo:RO_0001025 rdf:resource="http://purl.obolibrary.org/obo/GAZ_00002812"/>
        <obo:IAO_0000115>A game reserve located 280 km north of Durban.</obo:IAO_0000115>
        <oboInOwl:hasOBONamespace>GAZ</oboInOwl:hasOBONamespace>
        <oboInOwl:id>GAZ:00075413</oboInOwl:id>
        <rdfs:label>Hluhluwe-Umfolozi Game Reserve</rdfs:label>
    </owl:NamedIndividual>
    


    <!-- http://purl.obolibrary.org/obo/GAZ_00075414 -->

    <owl:NamedIndividual rdf:about="http://purl.obolibrary.org/obo/GAZ_00075414">
        <obo:RO_0001025 rdf:resource="http://purl.obolibrary.org/obo/GAZ_00005308"/>
        <obo:IAO_0000115>A national park within iSimangaliso Wetland Park.</obo:IAO_0000115>
        <oboInOwl:hasOBONamespace>GAZ</oboInOwl:hasOBONamespace>
        <oboInOwl:id>GAZ:00075414</oboInOwl:id>
        <rdfs:label>Sodwana Bay National Park</rdfs:label>
    </owl:NamedIndividual>
    


    <!-- http://purl.obolibrary.org/obo/GAZ_00075415 -->

    <owl:NamedIndividual rdf:about="http://purl.obolibrary.org/obo/GAZ_00075415">
        <obo:RO_0001025 rdf:resource="http://purl.obolibrary.org/obo/GAZ_00002812"/>
        <obo:IAO_0000115>A protected area of 290 km2 of rugged, mountainous thornveld in northern KwaZulu-Natal, about 400 km north of Durban.</obo:IAO_0000115>
        <oboInOwl:hasOBONamespace>GAZ</oboInOwl:hasOBONamespace>
        <oboInOwl:id>GAZ:00075415</oboInOwl:id>
        <rdfs:label>Itala Game Reserve</rdfs:label>
    </owl:NamedIndividual>
    


    <!-- http://purl.obolibrary.org/obo/GAZ_00075416 -->

    <owl:NamedIndividual rdf:about="http://purl.obolibrary.org/obo/GAZ_00075416">
        <obo:RO_0001025 rdf:resource="http://purl.obolibrary.org/obo/GAZ_00005308"/>
        <obo:IAO_0000115>A reserve that is located in northern Zululand, KwaZulu-Natal, South Africa.</obo:IAO_0000115>
        <oboInOwl:hasOBONamespace>GAZ</oboInOwl:hasOBONamespace>
        <oboInOwl:id>GAZ:00075416</oboInOwl:id>
        <rdfs:label>Mkuze Game Reserve</rdfs:label>
    </owl:NamedIndividual>
    


    <!-- http://purl.obolibrary.org/obo/GAZ_00075417 -->

    <owl:NamedIndividual rdf:about="http://purl.obolibrary.org/obo/GAZ_00075417">
        <obo:RO_0001025 rdf:resource="http://purl.obolibrary.org/obo/GAZ_00002812"/>
        <obo:IAO_0000115>A 170 km2 game reserve situated in KwaZulu-Natal, South Africa between the Mkuze Game Reserve and the Greater Saint Lucia Wetland Park. Established 1991.</obo:IAO_0000115>
        <oboInOwl:hasOBONamespace>GAZ</oboInOwl:hasOBONamespace>
        <oboInOwl:id>GAZ:00075417</oboInOwl:id>
        <rdfs:label>Phinda Resource Reserve</rdfs:label>
    </owl:NamedIndividual>
    


    <!-- http://purl.obolibrary.org/obo/GAZ_00075418 -->

    <owl:NamedIndividual rdf:about="http://purl.obolibrary.org/obo/GAZ_00075418">
        <obo:RO_0001025 rdf:resource="http://purl.obolibrary.org/obo/GAZ_00032881"/>
        <obo:IAO_0000115>A massif of approximately 15,000 km2 in north Limpopo Province, South Africa.</obo:IAO_0000115>
        <oboInOwl:hasOBONamespace>GAZ</oboInOwl:hasOBONamespace>
        <oboInOwl:id>GAZ:00075418</oboInOwl:id>
        <rdfs:label>Waterberg Biosphere</rdfs:label>
    </owl:NamedIndividual>
    


    <!-- http://purl.obolibrary.org/obo/GAZ_00075419 -->

    <owl:NamedIndividual rdf:about="http://purl.obolibrary.org/obo/GAZ_00075419">
        <obo:RO_0001025 rdf:resource="http://purl.obolibrary.org/obo/GAZ_00002818"/>
        <obo:IAO_0000115>A large wildlife preserve and conservation area in southern Africa. The park straddles the border between South Africa and Botswana and comprises two adjoining national parks: Kalahari Gemsbok National Park in South Africa and Gemsbok National Park in Botswana.</obo:IAO_0000115>
        <oboInOwl:hasOBONamespace>GAZ</oboInOwl:hasOBONamespace>
        <oboInOwl:id>GAZ:00075419</oboInOwl:id>
        <rdfs:label>Kgalagadi Transfrontier Park</rdfs:label>
    </owl:NamedIndividual>
    


    <!-- http://purl.obolibrary.org/obo/GAZ_00075420 -->

    <owl:NamedIndividual rdf:about="http://purl.obolibrary.org/obo/GAZ_00075420">
        <obo:RO_0001025 rdf:resource="http://purl.obolibrary.org/obo/GAZ_00075419"/>
        <obo:IAO_0000115>A national park in North West Province, Republic of South Africa.</obo:IAO_0000115>
        <oboInOwl:hasOBONamespace>GAZ</oboInOwl:hasOBONamespace>
        <oboInOwl:id>GAZ:00075420</oboInOwl:id>
        <rdfs:label>Kalahari Gemsbok National Park</rdfs:label>
    </owl:NamedIndividual>
    


    <!-- http://purl.obolibrary.org/obo/GAZ_00075421 -->

    <owl:NamedIndividual rdf:about="http://purl.obolibrary.org/obo/GAZ_00075421">
        <obo:RO_0001025 rdf:resource="http://purl.obolibrary.org/obo/GAZ_00075419"/>
        <obo:IAO_0000115>A national park in Botswana.</obo:IAO_0000115>
        <oboInOwl:hasOBONamespace>GAZ</oboInOwl:hasOBONamespace>
        <oboInOwl:id>GAZ:00075421</oboInOwl:id>
        <rdfs:label>Gemsbok National Park</rdfs:label>
    </owl:NamedIndividual>
    


    <!-- http://purl.obolibrary.org/obo/GAZ_00075422 -->

    <owl:NamedIndividual rdf:about="http://purl.obolibrary.org/obo/GAZ_00075422">
        <obo:IAO_0000115>A large salt pan complex in Northern Botswana, the largest salt flat complex in the world. These salt pans cover 16,000 km2 and form the bed of an ancient lake that started evaporating 10,000 years ago. The main water source is the Nata River, called Amanzinyama in Zimbabwe where it rises at Sandown about 60 km from Bulawayo.</obo:IAO_0000115>
        <oboInOwl:hasOBONamespace>GAZ</oboInOwl:hasOBONamespace>
        <oboInOwl:id>GAZ:00075422</oboInOwl:id>
        <rdfs:label>Makgadikgadi Pans</rdfs:label>
    </owl:NamedIndividual>
    


    <!-- http://purl.obolibrary.org/obo/GAZ_00075423 -->

    <owl:NamedIndividual rdf:about="http://purl.obolibrary.org/obo/GAZ_00075423">
        <obo:RO_0001025 rdf:resource="http://purl.obolibrary.org/obo/GAZ_00237428"/>
        <obo:IAO_0000115>A dry granite rock island located in the Makgadikgadi Pans National Park area of Botswana.</obo:IAO_0000115>
        <oboInOwl:hasOBONamespace>GAZ</oboInOwl:hasOBONamespace>
        <oboInOwl:id>GAZ:00075423</oboInOwl:id>
        <rdfs:label>Kubu Island</rdfs:label>
    </owl:NamedIndividual>
    


    <!-- http://purl.obolibrary.org/obo/GAZ_00075424 -->

    <owl:NamedIndividual rdf:about="http://purl.obolibrary.org/obo/GAZ_00075424">
        <obo:RO_0001025 rdf:resource="http://purl.obolibrary.org/obo/GAZ_00075422"/>
        <oboInOwl:hasOBONamespace>GAZ</oboInOwl:hasOBONamespace>
        <oboInOwl:id>GAZ:00075424</oboInOwl:id>
        <rdfs:label>Makgadikgadi Pans National Park</rdfs:label>
    </owl:NamedIndividual>
    


    <!-- http://purl.obolibrary.org/obo/GAZ_00075894 -->

    <owl:NamedIndividual rdf:about="http://purl.obolibrary.org/obo/GAZ_00075894">
        <obo:RO_0001025 rdf:resource="http://purl.obolibrary.org/obo/GAZ_00032892"/>
        <obo:IAO_0000115>A local municipality of Amajuba District Municipality in KwaZulu-Natal Province.</obo:IAO_0000115>
        <oboInOwl:hasOBONamespace>GAZ</oboInOwl:hasOBONamespace>
        <oboInOwl:id>GAZ:00075894</oboInOwl:id>
        <rdfs:label>eMadlangeni Local Municipality</rdfs:label>
    </owl:NamedIndividual>
    


    <!-- http://purl.obolibrary.org/obo/GAZ_00075895 -->

    <owl:NamedIndividual rdf:about="http://purl.obolibrary.org/obo/GAZ_00075895">
        <obo:RO_0001025 rdf:resource="http://purl.obolibrary.org/obo/GAZ_00032892"/>
        <obo:IAO_0000115>A local municipality of Amajuba District Municipality in KwaZulu-Natal Province.</obo:IAO_0000115>
        <oboInOwl:hasOBONamespace>GAZ</oboInOwl:hasOBONamespace>
        <oboInOwl:id>GAZ:00075895</oboInOwl:id>
        <rdfs:label>Dannhauser Local Municipality</rdfs:label>
    </owl:NamedIndividual>
    


    <!-- http://purl.obolibrary.org/obo/GAZ_00075896 -->

    <owl:NamedIndividual rdf:about="http://purl.obolibrary.org/obo/GAZ_00075896">
        <obo:RO_0001025 rdf:resource="http://purl.obolibrary.org/obo/GAZ_00032892"/>
        <obo:IAO_0000115>A local municipality of Amajuba District Municipality in KwaZulu-Natal Province.</obo:IAO_0000115>
        <oboInOwl:hasOBONamespace>GAZ</oboInOwl:hasOBONamespace>
        <oboInOwl:id>GAZ:00075896</oboInOwl:id>
        <rdfs:label>Newcastle Local Municipality</rdfs:label>
    </owl:NamedIndividual>
    


    <!-- http://purl.obolibrary.org/obo/GAZ_00075897 -->

    <owl:NamedIndividual rdf:about="http://purl.obolibrary.org/obo/GAZ_00075897">
        <obo:RO_0001025 rdf:resource="http://purl.obolibrary.org/obo/GAZ_00032894"/>
        <obo:IAO_0000115>A local municipality in Ugu District Municipality, KwaZulu-Natal.</obo:IAO_0000115>
        <oboInOwl:hasOBONamespace>GAZ</oboInOwl:hasOBONamespace>
        <oboInOwl:id>GAZ:00075897</oboInOwl:id>
        <rdfs:label>Hibiscus Coast Local Municipality</rdfs:label>
    </owl:NamedIndividual>
    


    <!-- http://purl.obolibrary.org/obo/GAZ_00075898 -->

    <owl:NamedIndividual rdf:about="http://purl.obolibrary.org/obo/GAZ_00075898">
        <obo:RO_0001025 rdf:resource="http://purl.obolibrary.org/obo/GAZ_00032894"/>
        <obo:IAO_0000115>A local municipality in Ugu District Municipality, KwaZulu-Natal.</obo:IAO_0000115>
        <oboInOwl:hasOBONamespace>GAZ</oboInOwl:hasOBONamespace>
        <oboInOwl:id>GAZ:00075898</oboInOwl:id>
        <rdfs:label>Vulamehlo Local Municipality</rdfs:label>
    </owl:NamedIndividual>
    


    <!-- http://purl.obolibrary.org/obo/GAZ_00075899 -->

    <owl:NamedIndividual rdf:about="http://purl.obolibrary.org/obo/GAZ_00075899">
        <obo:RO_0001025 rdf:resource="http://purl.obolibrary.org/obo/GAZ_00032894"/>
        <obo:IAO_0000115>A local municipality in Ugu District Municipality, KwaZulu-Natal.</obo:IAO_0000115>
        <oboInOwl:hasOBONamespace>GAZ</oboInOwl:hasOBONamespace>
        <oboInOwl:id>GAZ:00075899</oboInOwl:id>
        <rdfs:label>uMuziwabantu Local Municipality</rdfs:label>
    </owl:NamedIndividual>
    


    <!-- http://purl.obolibrary.org/obo/GAZ_00075900 -->

    <owl:NamedIndividual rdf:about="http://purl.obolibrary.org/obo/GAZ_00075900">
        <obo:RO_0001025 rdf:resource="http://purl.obolibrary.org/obo/GAZ_00032894"/>
        <obo:IAO_0000115>A local municipality in Ugu District Municipality, KwaZulu-Natal.</obo:IAO_0000115>
        <oboInOwl:hasOBONamespace>GAZ</oboInOwl:hasOBONamespace>
        <oboInOwl:id>GAZ:00075900</oboInOwl:id>
        <rdfs:label>Umzumbe Local Municipality</rdfs:label>
    </owl:NamedIndividual>
    


    <!-- http://purl.obolibrary.org/obo/GAZ_00075901 -->

    <owl:NamedIndividual rdf:about="http://purl.obolibrary.org/obo/GAZ_00075901">
        <obo:RO_0001025 rdf:resource="http://purl.obolibrary.org/obo/GAZ_00032894"/>
        <obo:IAO_0000115>A local municipality in Ugu District Municipality, KwaZulu-Natal.</obo:IAO_0000115>
        <oboInOwl:hasOBONamespace>GAZ</oboInOwl:hasOBONamespace>
        <oboInOwl:id>GAZ:00075901</oboInOwl:id>
        <rdfs:label>Umdoni Local Municipality</rdfs:label>
    </owl:NamedIndividual>
    


    <!-- http://purl.obolibrary.org/obo/GAZ_00075902 -->

    <owl:NamedIndividual rdf:about="http://purl.obolibrary.org/obo/GAZ_00075902">
        <obo:RO_0001025 rdf:resource="http://purl.obolibrary.org/obo/GAZ_00032894"/>
        <obo:IAO_0000115>A local municipality in Ugu District Municipality, KwaZulu-Natal.</obo:IAO_0000115>
        <oboInOwl:hasOBONamespace>GAZ</oboInOwl:hasOBONamespace>
        <oboInOwl:id>GAZ:00075902</oboInOwl:id>
        <rdfs:label>Ezingoleni Local Municipality</rdfs:label>
    </owl:NamedIndividual>
    


    <!-- http://purl.obolibrary.org/obo/GAZ_00075903 -->

    <owl:NamedIndividual rdf:about="http://purl.obolibrary.org/obo/GAZ_00075903">
        <obo:RO_0001025 rdf:resource="http://purl.obolibrary.org/obo/GAZ_00032890"/>
        <obo:IAO_0000115>A local municipality in Zululand District Municipality, KwaZulu-Natal.</obo:IAO_0000115>
        <oboInOwl:hasOBONamespace>GAZ</oboInOwl:hasOBONamespace>
        <oboInOwl:id>GAZ:00075903</oboInOwl:id>
        <rdfs:label>Ulundi Local Municipality</rdfs:label>
    </owl:NamedIndividual>
    


    <!-- http://purl.obolibrary.org/obo/GAZ_00075904 -->

    <owl:NamedIndividual rdf:about="http://purl.obolibrary.org/obo/GAZ_00075904">
        <obo:RO_0001025 rdf:resource="http://purl.obolibrary.org/obo/GAZ_00032890"/>
        <obo:IAO_0000115>A local municipality in Zululand District Municipality, KwaZulu-Natal.</obo:IAO_0000115>
        <oboInOwl:hasOBONamespace>GAZ</oboInOwl:hasOBONamespace>
        <oboInOwl:id>GAZ:00075904</oboInOwl:id>
        <rdfs:label>Nongoma Local Municipality</rdfs:label>
    </owl:NamedIndividual>
    


    <!-- http://purl.obolibrary.org/obo/GAZ_00075905 -->

    <owl:NamedIndividual rdf:about="http://purl.obolibrary.org/obo/GAZ_00075905">
        <obo:RO_0001025 rdf:resource="http://purl.obolibrary.org/obo/GAZ_00032890"/>
        <obo:IAO_0000115>A local municipality in Zululand District Municipality, KwaZulu-Natal.</obo:IAO_0000115>
        <oboInOwl:hasOBONamespace>GAZ</oboInOwl:hasOBONamespace>
        <oboInOwl:id>GAZ:00075905</oboInOwl:id>
        <rdfs:label>Abaqulusi Local Municipality</rdfs:label>
    </owl:NamedIndividual>
    


    <!-- http://purl.obolibrary.org/obo/GAZ_00075906 -->

    <owl:NamedIndividual rdf:about="http://purl.obolibrary.org/obo/GAZ_00075906">
        <obo:RO_0001025 rdf:resource="http://purl.obolibrary.org/obo/GAZ_00032890"/>
        <obo:IAO_0000115>A local municipality in Zululand District Municipality, KwaZulu-Natal.</obo:IAO_0000115>
        <oboInOwl:hasOBONamespace>GAZ</oboInOwl:hasOBONamespace>
        <oboInOwl:id>GAZ:00075906</oboInOwl:id>
        <rdfs:label>uPhongolo Local Municipality</rdfs:label>
    </owl:NamedIndividual>
    


    <!-- http://purl.obolibrary.org/obo/GAZ_00075907 -->

    <owl:NamedIndividual rdf:about="http://purl.obolibrary.org/obo/GAZ_00075907">
        <obo:RO_0001025 rdf:resource="http://purl.obolibrary.org/obo/GAZ_00032890"/>
        <obo:IAO_0000115>A local municipality in Zululand District Municipality, KwaZulu-Natal.</obo:IAO_0000115>
        <oboInOwl:hasOBONamespace>GAZ</oboInOwl:hasOBONamespace>
        <oboInOwl:id>GAZ:00075907</oboInOwl:id>
        <rdfs:label>eDumbe Local Municipality</rdfs:label>
    </owl:NamedIndividual>
    


    <!-- http://purl.obolibrary.org/obo/GAZ_00075908 -->

    <owl:NamedIndividual rdf:about="http://purl.obolibrary.org/obo/GAZ_00075908">
        <obo:RO_0001025 rdf:resource="http://purl.obolibrary.org/obo/GAZ_00032893"/>
        <obo:IAO_0000115>A local municipality in iLembe District Municipality, KwaZulu-Natal Province.</obo:IAO_0000115>
        <oboInOwl:hasOBONamespace>GAZ</oboInOwl:hasOBONamespace>
        <oboInOwl:id>GAZ:00075908</oboInOwl:id>
        <rdfs:label>eNdondakusuka Local Municipality</rdfs:label>
    </owl:NamedIndividual>
    


    <!-- http://purl.obolibrary.org/obo/GAZ_00075909 -->

    <owl:NamedIndividual rdf:about="http://purl.obolibrary.org/obo/GAZ_00075909">
        <obo:RO_0001025 rdf:resource="http://purl.obolibrary.org/obo/GAZ_00032893"/>
        <obo:IAO_0000115>A local municipality in iLembe District Municipality, KwaZulu-Natal Province.</obo:IAO_0000115>
        <oboInOwl:hasOBONamespace>GAZ</oboInOwl:hasOBONamespace>
        <oboInOwl:id>GAZ:00075909</oboInOwl:id>
        <rdfs:label>Ndwedwe Local Municipality</rdfs:label>
    </owl:NamedIndividual>
    


    <!-- http://purl.obolibrary.org/obo/GAZ_00075910 -->

    <owl:NamedIndividual rdf:about="http://purl.obolibrary.org/obo/GAZ_00075910">
        <obo:RO_0001025 rdf:resource="http://purl.obolibrary.org/obo/GAZ_00032893"/>
        <obo:IAO_0000115>A local municipality in iLembe District Municipality, KwaZulu-Natal Province.</obo:IAO_0000115>
        <oboInOwl:hasOBONamespace>GAZ</oboInOwl:hasOBONamespace>
        <oboInOwl:id>GAZ:00075910</oboInOwl:id>
        <rdfs:label>KwaDukuza Local Municipality</rdfs:label>
    </owl:NamedIndividual>
    


    <!-- http://purl.obolibrary.org/obo/GAZ_00075911 -->

    <owl:NamedIndividual rdf:about="http://purl.obolibrary.org/obo/GAZ_00075911">
        <obo:RO_0001025 rdf:resource="http://purl.obolibrary.org/obo/GAZ_00032893"/>
        <obo:IAO_0000115>A local municipality in iLembe District Municipality, KwaZulu-Natal Province.</obo:IAO_0000115>
        <oboInOwl:hasOBONamespace>GAZ</oboInOwl:hasOBONamespace>
        <oboInOwl:id>GAZ:00075911</oboInOwl:id>
        <rdfs:label>Maphumulo Local Municipality</rdfs:label>
    </owl:NamedIndividual>
    


    <!-- http://purl.obolibrary.org/obo/GAZ_00075912 -->

    <owl:NamedIndividual rdf:about="http://purl.obolibrary.org/obo/GAZ_00075912">
        <obo:RO_0001025 rdf:resource="http://purl.obolibrary.org/obo/GAZ_00012787"/>
        <obo:IAO_0000115>A local municipality in Sisonke District Municipality, KwaZulu-Natal Province.</obo:IAO_0000115>
        <oboInOwl:hasOBONamespace>GAZ</oboInOwl:hasOBONamespace>
        <oboInOwl:id>GAZ:00075912</oboInOwl:id>
        <rdfs:label>Kwa Sani Local Municipality</rdfs:label>
    </owl:NamedIndividual>
    


    <!-- http://purl.obolibrary.org/obo/GAZ_00075913 -->

    <owl:NamedIndividual rdf:about="http://purl.obolibrary.org/obo/GAZ_00075913">
        <obo:RO_0001025 rdf:resource="http://purl.obolibrary.org/obo/GAZ_00012787"/>
        <obo:IAO_0000115>A local municipality in Sisonke District Municipality, KwaZulu-Natal Province.</obo:IAO_0000115>
        <oboInOwl:hasOBONamespace>GAZ</oboInOwl:hasOBONamespace>
        <oboInOwl:id>GAZ:00075913</oboInOwl:id>
        <rdfs:label>Ingwe Local Municipality</rdfs:label>
    </owl:NamedIndividual>
    


    <!-- http://purl.obolibrary.org/obo/GAZ_00075914 -->

    <owl:NamedIndividual rdf:about="http://purl.obolibrary.org/obo/GAZ_00075914">
        <obo:RO_0001025 rdf:resource="http://purl.obolibrary.org/obo/GAZ_00012787"/>
        <obo:IAO_0000115>A local municipality in Sisonke District Municipality, KwaZulu-Natal Province.</obo:IAO_0000115>
        <oboInOwl:hasOBONamespace>GAZ</oboInOwl:hasOBONamespace>
        <oboInOwl:id>GAZ:00075914</oboInOwl:id>
        <rdfs:label>Ubuhlebezwe Local Municipality</rdfs:label>
    </owl:NamedIndividual>
    


    <!-- http://purl.obolibrary.org/obo/GAZ_00075915 -->

    <owl:NamedIndividual rdf:about="http://purl.obolibrary.org/obo/GAZ_00075915">
        <obo:RO_0001025 rdf:resource="http://purl.obolibrary.org/obo/GAZ_00012787"/>
        <obo:IAO_0000115>A District Management Area in Sisonke District Municipality, KwaZulu-Natal Province.</obo:IAO_0000115>
        <oboInOwl:hasOBONamespace>GAZ</oboInOwl:hasOBONamespace>
        <oboInOwl:id>GAZ:00075915</oboInOwl:id>
        <rdfs:label>Mkhomazi Wilderness Area</rdfs:label>
    </owl:NamedIndividual>
    


    <!-- http://purl.obolibrary.org/obo/GAZ_00075916 -->

    <owl:NamedIndividual rdf:about="http://purl.obolibrary.org/obo/GAZ_00075916">
        <obo:RO_0001025 rdf:resource="http://purl.obolibrary.org/obo/GAZ_00012787"/>
        <obo:IAO_0000115>A local municipality in Sisonke District Municipality, KwaZulu-Natal Province.</obo:IAO_0000115>
        <oboInOwl:hasOBONamespace>GAZ</oboInOwl:hasOBONamespace>
        <oboInOwl:id>GAZ:00075916</oboInOwl:id>
        <rdfs:label>Greater Kokstad Local Municipality</rdfs:label>
    </owl:NamedIndividual>
    


    <!-- http://purl.obolibrary.org/obo/GAZ_00075917 -->

    <owl:NamedIndividual rdf:about="http://purl.obolibrary.org/obo/GAZ_00075917">
        <obo:RO_0001025 rdf:resource="http://purl.obolibrary.org/obo/GAZ_00032891"/>
        <obo:IAO_0000115>A local municipality in uThungulu District Municipality, KwaZulu-Natal Province.</obo:IAO_0000115>
        <oboInOwl:hasOBONamespace>GAZ</oboInOwl:hasOBONamespace>
        <oboInOwl:id>GAZ:00075917</oboInOwl:id>
        <rdfs:label>Nkandla Local Municipality</rdfs:label>
    </owl:NamedIndividual>
    


    <!-- http://purl.obolibrary.org/obo/GAZ_00075918 -->

    <owl:NamedIndividual rdf:about="http://purl.obolibrary.org/obo/GAZ_00075918">
        <obo:RO_0001025 rdf:resource="http://purl.obolibrary.org/obo/GAZ_00032891"/>
        <obo:IAO_0000115>A local municipality in uThungulu District Municipality, KwaZulu-Natal Province.</obo:IAO_0000115>
        <oboInOwl:hasOBONamespace>GAZ</oboInOwl:hasOBONamespace>
        <oboInOwl:id>GAZ:00075918</oboInOwl:id>
        <rdfs:label>Ntambanana Local Municipality</rdfs:label>
    </owl:NamedIndividual>
    


    <!-- http://purl.obolibrary.org/obo/GAZ_00075919 -->

    <owl:NamedIndividual rdf:about="http://purl.obolibrary.org/obo/GAZ_00075919">
        <obo:RO_0001025 rdf:resource="http://purl.obolibrary.org/obo/GAZ_00032891"/>
        <obo:IAO_0000115>A local municipality in uThungulu District Municipality, KwaZulu-Natal Province.</obo:IAO_0000115>
        <oboInOwl:hasOBONamespace>GAZ</oboInOwl:hasOBONamespace>
        <oboInOwl:id>GAZ:00075919</oboInOwl:id>
        <rdfs:label>uMhlathuze Local Municipality</rdfs:label>
    </owl:NamedIndividual>
    


    <!-- http://purl.obolibrary.org/obo/GAZ_00075920 -->

    <owl:NamedIndividual rdf:about="http://purl.obolibrary.org/obo/GAZ_00075920">
        <obo:RO_0001025 rdf:resource="http://purl.obolibrary.org/obo/GAZ_00032891"/>
        <obo:IAO_0000115>A local municipality in uThungulu District Municipality, KwaZulu-Natal Province.</obo:IAO_0000115>
        <oboInOwl:hasOBONamespace>GAZ</oboInOwl:hasOBONamespace>
        <oboInOwl:id>GAZ:00075920</oboInOwl:id>
        <rdfs:label>Mbonambi Local Municipality</rdfs:label>
    </owl:NamedIndividual>
    


    <!-- http://purl.obolibrary.org/obo/GAZ_00075921 -->

    <owl:NamedIndividual rdf:about="http://purl.obolibrary.org/obo/GAZ_00075921">
        <obo:RO_0001025 rdf:resource="http://purl.obolibrary.org/obo/GAZ_00032891"/>
        <obo:IAO_0000115>A local municipality in uThungulu District Municipality, KwaZulu-Natal Province.</obo:IAO_0000115>
        <oboInOwl:hasOBONamespace>GAZ</oboInOwl:hasOBONamespace>
        <oboInOwl:id>GAZ:00075921</oboInOwl:id>
        <rdfs:label>Mthonjaneni Local Municipality</rdfs:label>
    </owl:NamedIndividual>
    


    <!-- http://purl.obolibrary.org/obo/GAZ_00075922 -->

    <owl:NamedIndividual rdf:about="http://purl.obolibrary.org/obo/GAZ_00075922">
        <obo:RO_0001025 rdf:resource="http://purl.obolibrary.org/obo/GAZ_00032891"/>
        <obo:IAO_0000115>A local municipality in uThungulu District Municipality, KwaZulu-Natal Province.</obo:IAO_0000115>
        <oboInOwl:hasOBONamespace>GAZ</oboInOwl:hasOBONamespace>
        <oboInOwl:id>GAZ:00075922</oboInOwl:id>
        <rdfs:label>uMlalazi Local Municipality</rdfs:label>
    </owl:NamedIndividual>
    


    <!-- http://purl.obolibrary.org/obo/GAZ_00075923 -->

    <owl:NamedIndividual rdf:about="http://purl.obolibrary.org/obo/GAZ_00075923">
        <obo:RO_0001025 rdf:resource="http://purl.obolibrary.org/obo/GAZ_00008040"/>
        <obo:IAO_0000115>A local municipality in Umgungundlovu District Municipality, KwaZulu-Natal.</obo:IAO_0000115>
        <oboInOwl:hasOBONamespace>GAZ</oboInOwl:hasOBONamespace>
        <oboInOwl:id>GAZ:00075923</oboInOwl:id>
        <rdfs:label>Mkhambathini Local Municipality</rdfs:label>
    </owl:NamedIndividual>
    


    <!-- http://purl.obolibrary.org/obo/GAZ_00075924 -->

    <owl:NamedIndividual rdf:about="http://purl.obolibrary.org/obo/GAZ_00075924">
        <obo:RO_0001025 rdf:resource="http://purl.obolibrary.org/obo/GAZ_00008040"/>
        <obo:IAO_0000115>A local municipality in Umgungundlovu District Municipality, KwaZulu-Natal.</obo:IAO_0000115>
        <oboInOwl:hasOBONamespace>GAZ</oboInOwl:hasOBONamespace>
        <oboInOwl:id>GAZ:00075924</oboInOwl:id>
        <rdfs:label>uMngeni Local Municipality</rdfs:label>
    </owl:NamedIndividual>
    


    <!-- http://purl.obolibrary.org/obo/GAZ_00075925 -->

    <owl:NamedIndividual rdf:about="http://purl.obolibrary.org/obo/GAZ_00075925">
        <obo:RO_0001025 rdf:resource="http://purl.obolibrary.org/obo/GAZ_00008040"/>
        <obo:IAO_0000115>A local municipality in Umgungundlovu District Municipality, KwaZulu-Natal.</obo:IAO_0000115>
        <oboInOwl:hasOBONamespace>GAZ</oboInOwl:hasOBONamespace>
        <oboInOwl:id>GAZ:00075925</oboInOwl:id>
        <rdfs:label>Impendle Local Municipality</rdfs:label>
    </owl:NamedIndividual>
    


    <!-- http://purl.obolibrary.org/obo/GAZ_00075926 -->

    <owl:NamedIndividual rdf:about="http://purl.obolibrary.org/obo/GAZ_00075926">
        <obo:RO_0001025 rdf:resource="http://purl.obolibrary.org/obo/GAZ_00008040"/>
        <obo:IAO_0000115>A local municipality in Umgungundlovu District Municipality, KwaZulu-Natal.</obo:IAO_0000115>
        <oboInOwl:hasOBONamespace>GAZ</oboInOwl:hasOBONamespace>
        <oboInOwl:id>GAZ:00075926</oboInOwl:id>
        <rdfs:label>uMshwathi Local Municipality</rdfs:label>
    </owl:NamedIndividual>
    


    <!-- http://purl.obolibrary.org/obo/GAZ_00075927 -->

    <owl:NamedIndividual rdf:about="http://purl.obolibrary.org/obo/GAZ_00075927">
        <obo:RO_0001025 rdf:resource="http://purl.obolibrary.org/obo/GAZ_00008040"/>
        <obo:IAO_0000115>A local municipality in Umgungundlovu District Municipality, KwaZulu-Natal.</obo:IAO_0000115>
        <oboInOwl:hasOBONamespace>GAZ</oboInOwl:hasOBONamespace>
        <oboInOwl:id>GAZ:00075927</oboInOwl:id>
        <rdfs:label>Richmond Local Municipality</rdfs:label>
    </owl:NamedIndividual>
    


    <!-- http://purl.obolibrary.org/obo/GAZ_00075928 -->

    <owl:NamedIndividual rdf:about="http://purl.obolibrary.org/obo/GAZ_00075928">
        <obo:RO_0001025 rdf:resource="http://purl.obolibrary.org/obo/GAZ_00008040"/>
        <obo:IAO_0000115>A local municipality in Umgungundlovu District Municipality, KwaZulu-Natal. It surrounds Pietermaritzburg.</obo:IAO_0000115>
        <oboInOwl:hasOBONamespace>GAZ</oboInOwl:hasOBONamespace>
        <oboInOwl:id>GAZ:00075928</oboInOwl:id>
        <rdfs:label>Msunduzi Local Municipality</rdfs:label>
    </owl:NamedIndividual>
    


    <!-- http://purl.obolibrary.org/obo/GAZ_00075929 -->

    <owl:NamedIndividual rdf:about="http://purl.obolibrary.org/obo/GAZ_00075929">
        <obo:RO_0001025 rdf:resource="http://purl.obolibrary.org/obo/GAZ_00008040"/>
        <obo:IAO_0000115>A local municipality in Umgungundlovu District Municipality, KwaZulu-Natal.</obo:IAO_0000115>
        <oboInOwl:hasOBONamespace>GAZ</oboInOwl:hasOBONamespace>
        <oboInOwl:id>GAZ:00075929</oboInOwl:id>
        <rdfs:label>Mooi Mpofana Local Municipality</rdfs:label>
    </owl:NamedIndividual>
    


    <!-- http://purl.obolibrary.org/obo/GAZ_00075930 -->

    <owl:NamedIndividual rdf:about="http://purl.obolibrary.org/obo/GAZ_00075930">
        <obo:RO_0001025 rdf:resource="http://purl.obolibrary.org/obo/GAZ_00008040"/>
        <obo:IAO_0000115>A District Management Area in Umgungundlovu District Municipality, KwaZulu-Natal.</obo:IAO_0000115>
        <oboInOwl:hasOBONamespace>GAZ</oboInOwl:hasOBONamespace>
        <oboInOwl:id>GAZ:00075930</oboInOwl:id>
        <rdfs:label>Highmoor/Kamberg Park</rdfs:label>
    </owl:NamedIndividual>
    


    <!-- http://purl.obolibrary.org/obo/GAZ_00075931 -->

    <owl:NamedIndividual rdf:about="http://purl.obolibrary.org/obo/GAZ_00075931">
        <obo:RO_0001025 rdf:resource="http://purl.obolibrary.org/obo/GAZ_00002812"/>
        <obo:IAO_0000115>One of the 11 districts of KwaZulu-Natal province of South Africa. The seat of Umkhanyakude is Mkuze.</obo:IAO_0000115>
        <oboInOwl:hasOBONamespace>GAZ</oboInOwl:hasOBONamespace>
        <oboInOwl:id>GAZ:00075931</oboInOwl:id>
        <rdfs:label>Umkhanyakude District Municipality</rdfs:label>
    </owl:NamedIndividual>
    


    <!-- http://purl.obolibrary.org/obo/GAZ_00075932 -->

    <owl:NamedIndividual rdf:about="http://purl.obolibrary.org/obo/GAZ_00075932">
        <obo:RO_0001025 rdf:resource="http://purl.obolibrary.org/obo/GAZ_00075931"/>
        <obo:IAO_0000115>A local municipality in Umkhanyakude District Municipality, KwaZulu-Natal Province.</obo:IAO_0000115>
        <oboInOwl:hasOBONamespace>GAZ</oboInOwl:hasOBONamespace>
        <oboInOwl:id>GAZ:00075932</oboInOwl:id>
        <rdfs:label>Umhlabuyalingana Local Municipality</rdfs:label>
    </owl:NamedIndividual>
    


    <!-- http://purl.obolibrary.org/obo/GAZ_00075933 -->

    <owl:NamedIndividual rdf:about="http://purl.obolibrary.org/obo/GAZ_00075933">
        <obo:RO_0001025 rdf:resource="http://purl.obolibrary.org/obo/GAZ_00075931"/>
        <obo:IAO_0000115>A local municipality in Umkhanyakude District Municipality, KwaZulu-Natal Province.</obo:IAO_0000115>
        <oboInOwl:hasOBONamespace>GAZ</oboInOwl:hasOBONamespace>
        <oboInOwl:id>GAZ:00075933</oboInOwl:id>
        <rdfs:label>Hlabisa Local Municipality</rdfs:label>
    </owl:NamedIndividual>
    


    <!-- http://purl.obolibrary.org/obo/GAZ_00075934 -->

    <owl:NamedIndividual rdf:about="http://purl.obolibrary.org/obo/GAZ_00075934">
        <obo:RO_0001025 rdf:resource="http://purl.obolibrary.org/obo/GAZ_00075931"/>
        <obo:IAO_0000115>A local municipality in Umkhanyakude District Municipality, KwaZulu-Natal Province.</obo:IAO_0000115>
        <oboInOwl:hasOBONamespace>GAZ</oboInOwl:hasOBONamespace>
        <oboInOwl:id>GAZ:00075934</oboInOwl:id>
        <rdfs:label>Mtubatuba Local Municipality</rdfs:label>
    </owl:NamedIndividual>
    


    <!-- http://purl.obolibrary.org/obo/GAZ_00075935 -->

    <owl:NamedIndividual rdf:about="http://purl.obolibrary.org/obo/GAZ_00075935">
        <obo:RO_0001025 rdf:resource="http://purl.obolibrary.org/obo/GAZ_00075931"/>
        <obo:IAO_0000115>A local municipality in Umkhanyakude District Municipality, KwaZulu-Natal Province.</obo:IAO_0000115>
        <oboInOwl:hasOBONamespace>GAZ</oboInOwl:hasOBONamespace>
        <oboInOwl:id>GAZ:00075935</oboInOwl:id>
        <rdfs:label>The Big Five False Bay Local Municipality</rdfs:label>
    </owl:NamedIndividual>
    


    <!-- http://purl.obolibrary.org/obo/GAZ_00075936 -->

    <owl:NamedIndividual rdf:about="http://purl.obolibrary.org/obo/GAZ_00075936">
        <obo:RO_0001025 rdf:resource="http://purl.obolibrary.org/obo/GAZ_00075931"/>
        <obo:IAO_0000115>A local municipality in Umkhanyakude District Municipality, KwaZulu-Natal Province.</obo:IAO_0000115>
        <oboInOwl:hasOBONamespace>GAZ</oboInOwl:hasOBONamespace>
        <oboInOwl:id>GAZ:00075936</oboInOwl:id>
        <rdfs:label>Jozini Local Municipality</rdfs:label>
    </owl:NamedIndividual>
    


    <!-- http://purl.obolibrary.org/obo/GAZ_00075937 -->

    <owl:NamedIndividual rdf:about="http://purl.obolibrary.org/obo/GAZ_00075937">
        <obo:RO_0001025 rdf:resource="http://purl.obolibrary.org/obo/GAZ_00075931"/>
        <obo:IAO_0000115>A District Management Area in Umkhanyakude District Municipality, KwaZulu-Natal Province.</obo:IAO_0000115>
        <oboInOwl:hasOBONamespace>GAZ</oboInOwl:hasOBONamespace>
        <oboInOwl:id>GAZ:00075937</oboInOwl:id>
        <rdfs:label>Saint Lucia Park</rdfs:label>
    </owl:NamedIndividual>
    


    <!-- http://purl.obolibrary.org/obo/GAZ_00075938 -->

    <owl:NamedIndividual rdf:about="http://purl.obolibrary.org/obo/GAZ_00075938">
        <obo:RO_0001025 rdf:resource="http://purl.obolibrary.org/obo/GAZ_00032888"/>
        <obo:IAO_0000115>A local municipality in Umzinyathi District Municipality, KwaZulu-Natal Province.</obo:IAO_0000115>
        <oboInOwl:hasOBONamespace>GAZ</oboInOwl:hasOBONamespace>
        <oboInOwl:id>GAZ:00075938</oboInOwl:id>
        <rdfs:label>Nqutu Local Municipality</rdfs:label>
    </owl:NamedIndividual>
    


    <!-- http://purl.obolibrary.org/obo/GAZ_00075939 -->

    <owl:NamedIndividual rdf:about="http://purl.obolibrary.org/obo/GAZ_00075939">
        <obo:RO_0001025 rdf:resource="http://purl.obolibrary.org/obo/GAZ_00032888"/>
        <obo:IAO_0000115>A local municipality in Umzinyathi District Municipality, KwaZulu-Natal Province.</obo:IAO_0000115>
        <oboInOwl:hasOBONamespace>GAZ</oboInOwl:hasOBONamespace>
        <oboInOwl:id>GAZ:00075939</oboInOwl:id>
        <rdfs:label>Endumeni Local Municipality</rdfs:label>
    </owl:NamedIndividual>
    


    <!-- http://purl.obolibrary.org/obo/GAZ_00075940 -->

    <owl:NamedIndividual rdf:about="http://purl.obolibrary.org/obo/GAZ_00075940">
        <obo:RO_0001025 rdf:resource="http://purl.obolibrary.org/obo/GAZ_00032888"/>
        <obo:IAO_0000115>A local municipality in Umzinyathi District Municipality, KwaZulu-Natal Province.</obo:IAO_0000115>
        <oboInOwl:hasOBONamespace>GAZ</oboInOwl:hasOBONamespace>
        <oboInOwl:id>GAZ:00075940</oboInOwl:id>
        <rdfs:label>Umvoti Local Municipality</rdfs:label>
    </owl:NamedIndividual>
    


    <!-- http://purl.obolibrary.org/obo/GAZ_00075941 -->

    <owl:NamedIndividual rdf:about="http://purl.obolibrary.org/obo/GAZ_00075941">
        <obo:RO_0001025 rdf:resource="http://purl.obolibrary.org/obo/GAZ_00032888"/>
        <obo:IAO_0000115>A local municipality in Umzinyathi District Municipality, KwaZulu-Natal Province.</obo:IAO_0000115>
        <oboInOwl:hasOBONamespace>GAZ</oboInOwl:hasOBONamespace>
        <oboInOwl:id>GAZ:00075941</oboInOwl:id>
        <rdfs:label>Msinga Local Municipality</rdfs:label>
    </owl:NamedIndividual>
    


    <!-- http://purl.obolibrary.org/obo/GAZ_00075942 -->

    <owl:NamedIndividual rdf:about="http://purl.obolibrary.org/obo/GAZ_00075942">
        <rdf:type rdf:resource="http://purl.obolibrary.org/obo/ENVO_00000856"/>
        <obo:RO_0001025 rdf:resource="http://purl.obolibrary.org/obo/GAZ_00032889"/>
        <obo:IAO_0000115>A municipality in the Uthukela District Municipality, KwaZulu-Natal, South Africa.</obo:IAO_0000115>
        <oboInOwl:hasOBONamespace>GAZ</oboInOwl:hasOBONamespace>
        <oboInOwl:id>GAZ:00075942</oboInOwl:id>
        <rdfs:label>Imbabazane Local Municipality</rdfs:label>
    </owl:NamedIndividual>
    


    <!-- http://purl.obolibrary.org/obo/GAZ_00075943 -->

    <owl:NamedIndividual rdf:about="http://purl.obolibrary.org/obo/GAZ_00075943">
        <rdf:type rdf:resource="http://purl.obolibrary.org/obo/ENVO_00000856"/>
        <obo:RO_0001025 rdf:resource="http://purl.obolibrary.org/obo/GAZ_00032889"/>
        <obo:IAO_0000115>A municipality in the Uthukela District Municipality, KwaZulu-Natal, South Africa.</obo:IAO_0000115>
        <oboInOwl:hasOBONamespace>GAZ</oboInOwl:hasOBONamespace>
        <oboInOwl:id>GAZ:00075943</oboInOwl:id>
        <rdfs:label>Indaka Local Municipality</rdfs:label>
    </owl:NamedIndividual>
    


    <!-- http://purl.obolibrary.org/obo/GAZ_00075944 -->

    <owl:NamedIndividual rdf:about="http://purl.obolibrary.org/obo/GAZ_00075944">
        <rdf:type rdf:resource="http://purl.obolibrary.org/obo/ENVO_00000856"/>
        <obo:RO_0001025 rdf:resource="http://purl.obolibrary.org/obo/GAZ_00032889"/>
        <obo:IAO_0000115>A municipality in the Uthukela District Municipality, KwaZulu-Natal, South Africa.</obo:IAO_0000115>
        <oboInOwl:hasOBONamespace>GAZ</oboInOwl:hasOBONamespace>
        <oboInOwl:id>GAZ:00075944</oboInOwl:id>
        <rdfs:label>Emnambithi-Ladysmith Local Municipality</rdfs:label>
    </owl:NamedIndividual>
    


    <!-- http://purl.obolibrary.org/obo/GAZ_00075945 -->

    <owl:NamedIndividual rdf:about="http://purl.obolibrary.org/obo/GAZ_00075945">
        <rdf:type rdf:resource="http://purl.obolibrary.org/obo/ENVO_00000856"/>
        <obo:RO_0001025 rdf:resource="http://purl.obolibrary.org/obo/GAZ_00032889"/>
        <obo:IAO_0000115>A municipality in the Uthukela District Municipality, KwaZulu-Natal, South Africa.</obo:IAO_0000115>
        <oboInOwl:hasOBONamespace>GAZ</oboInOwl:hasOBONamespace>
        <oboInOwl:id>GAZ:00075945</oboInOwl:id>
        <rdfs:label>Okhahlamba Local Municipality</rdfs:label>
    </owl:NamedIndividual>
    


    <!-- http://purl.obolibrary.org/obo/GAZ_00075946 -->

    <owl:NamedIndividual rdf:about="http://purl.obolibrary.org/obo/GAZ_00075946">
        <obo:RO_0001025 rdf:resource="http://purl.obolibrary.org/obo/GAZ_00032889"/>
        <obo:IAO_0000115>A District Management Area in the Uthukela District Municipality, KwaZulu-Natal, South Africa.</obo:IAO_0000115>
        <oboInOwl:hasOBONamespace>GAZ</oboInOwl:hasOBONamespace>
        <oboInOwl:id>GAZ:00075946</oboInOwl:id>
        <rdfs:label>Giants Castle Game Reserve</rdfs:label>
    </owl:NamedIndividual>
    


    <!-- http://purl.obolibrary.org/obo/GAZ_00075947 -->

    <owl:NamedIndividual rdf:about="http://purl.obolibrary.org/obo/GAZ_00075947">
        <rdf:type rdf:resource="http://purl.obolibrary.org/obo/ENVO_00000856"/>
        <obo:RO_0001025 rdf:resource="http://purl.obolibrary.org/obo/GAZ_00032889"/>
        <obo:IAO_0000115>A municipality in the Uthukela District Municipality, KwaZulu-Natal, South Africa.</obo:IAO_0000115>
        <oboInOwl:hasOBONamespace>GAZ</oboInOwl:hasOBONamespace>
        <oboInOwl:id>GAZ:00075947</oboInOwl:id>
        <rdfs:label>Umtshezi Local Municipality</rdfs:label>
    </owl:NamedIndividual>
    


    <!-- http://purl.obolibrary.org/obo/GAZ_00075948 -->

    <owl:NamedIndividual rdf:about="http://purl.obolibrary.org/obo/GAZ_00075948">
        <obo:RO_0001025 rdf:resource="http://purl.obolibrary.org/obo/GAZ_00032858"/>
        <obo:IAO_0000115>A local municipality in Cacadu District Municipality, Eastern Cape.</obo:IAO_0000115>
        <oboInOwl:hasOBONamespace>GAZ</oboInOwl:hasOBONamespace>
        <oboInOwl:id>GAZ:00075948</oboInOwl:id>
        <rdfs:label>Makana Local Municipality</rdfs:label>
    </owl:NamedIndividual>
    


    <!-- http://purl.obolibrary.org/obo/GAZ_00075949 -->

    <owl:NamedIndividual rdf:about="http://purl.obolibrary.org/obo/GAZ_00075949">
        <obo:RO_0001025 rdf:resource="http://purl.obolibrary.org/obo/GAZ_00032858"/>
        <obo:IAO_0000115>A local municipality in Cacadu District Municipality, Eastern Cape.</obo:IAO_0000115>
        <oboInOwl:hasOBONamespace>GAZ</oboInOwl:hasOBONamespace>
        <oboInOwl:id>GAZ:00075949</oboInOwl:id>
        <rdfs:label>Ikwezi Local Municipality</rdfs:label>
    </owl:NamedIndividual>
    


    <!-- http://purl.obolibrary.org/obo/GAZ_00075950 -->

    <owl:NamedIndividual rdf:about="http://purl.obolibrary.org/obo/GAZ_00075950">
        <obo:RO_0001025 rdf:resource="http://purl.obolibrary.org/obo/GAZ_00032858"/>
        <obo:IAO_0000115>A local municipality in Cacadu District Municipality, Eastern Cape.</obo:IAO_0000115>
        <oboInOwl:hasOBONamespace>GAZ</oboInOwl:hasOBONamespace>
        <oboInOwl:id>GAZ:00075950</oboInOwl:id>
        <rdfs:label>Kou-Kamma Local Municipality</rdfs:label>
    </owl:NamedIndividual>
    


    <!-- http://purl.obolibrary.org/obo/GAZ_00075951 -->

    <owl:NamedIndividual rdf:about="http://purl.obolibrary.org/obo/GAZ_00075951">
        <obo:RO_0001025 rdf:resource="http://purl.obolibrary.org/obo/GAZ_00032858"/>
        <obo:IAO_0000115>A local municipality in the Eastern Cape of South Africa, with its capital at Port Alfred.</obo:IAO_0000115>
        <oboInOwl:hasOBONamespace>GAZ</oboInOwl:hasOBONamespace>
        <oboInOwl:id>GAZ:00075951</oboInOwl:id>
        <rdfs:label>Ndlambe Local Municipality</rdfs:label>
    </owl:NamedIndividual>
    


    <!-- http://purl.obolibrary.org/obo/GAZ_00075952 -->

    <owl:NamedIndividual rdf:about="http://purl.obolibrary.org/obo/GAZ_00075952">
        <obo:RO_0001025 rdf:resource="http://purl.obolibrary.org/obo/GAZ_00032858"/>
        <obo:IAO_0000115>A local municipality in Cacadu District Municipality, Eastern Cape.</obo:IAO_0000115>
        <oboInOwl:hasOBONamespace>GAZ</oboInOwl:hasOBONamespace>
        <oboInOwl:id>GAZ:00075952</oboInOwl:id>
        <rdfs:label>Baviaans Local Municipality</rdfs:label>
    </owl:NamedIndividual>
    


    <!-- http://purl.obolibrary.org/obo/GAZ_00075953 -->

    <owl:NamedIndividual rdf:about="http://purl.obolibrary.org/obo/GAZ_00075953">
        <obo:RO_0001025 rdf:resource="http://purl.obolibrary.org/obo/GAZ_00032858"/>
        <obo:IAO_0000115>A local municipality in Cacadu District Municipality, Eastern Cape.</obo:IAO_0000115>
        <oboInOwl:hasOBONamespace>GAZ</oboInOwl:hasOBONamespace>
        <oboInOwl:id>GAZ:00075953</oboInOwl:id>
        <rdfs:label>Blue Crane Route Local Municipality</rdfs:label>
    </owl:NamedIndividual>
    


    <!-- http://purl.obolibrary.org/obo/GAZ_00075954 -->

    <owl:NamedIndividual rdf:about="http://purl.obolibrary.org/obo/GAZ_00075954">
        <obo:RO_0001025 rdf:resource="http://purl.obolibrary.org/obo/GAZ_00032858"/>
        <obo:IAO_0000115>A local municipality in Cacadu District Municipality, Eastern Cape.</obo:IAO_0000115>
        <oboInOwl:hasOBONamespace>GAZ</oboInOwl:hasOBONamespace>
        <oboInOwl:id>GAZ:00075954</oboInOwl:id>
        <rdfs:label>Camdeboo Local Municipality</rdfs:label>
    </owl:NamedIndividual>
    


    <!-- http://purl.obolibrary.org/obo/GAZ_00075955 -->

    <owl:NamedIndividual rdf:about="http://purl.obolibrary.org/obo/GAZ_00075955">
        <obo:RO_0001025 rdf:resource="http://purl.obolibrary.org/obo/GAZ_00032858"/>
        <obo:IAO_0000115>A local municipality in Cacadu District Municipality, Eastern Cape. The seat of Sunday&apos;s River Valley is Kirkwood.</obo:IAO_0000115>
        <oboInOwl:hasOBONamespace>GAZ</oboInOwl:hasOBONamespace>
        <oboInOwl:id>GAZ:00075955</oboInOwl:id>
        <rdfs:label>Sunday&apos;s River Valley Local Municipality</rdfs:label>
    </owl:NamedIndividual>
    


    <!-- http://purl.obolibrary.org/obo/GAZ_00075956 -->

    <owl:NamedIndividual rdf:about="http://purl.obolibrary.org/obo/GAZ_00075956">
        <obo:RO_0001025 rdf:resource="http://purl.obolibrary.org/obo/GAZ_00032858"/>
        <obo:IAO_0000115>A local municipality in Cacadu District Municipality, Eastern Cape.</obo:IAO_0000115>
        <oboInOwl:hasOBONamespace>GAZ</oboInOwl:hasOBONamespace>
        <oboInOwl:id>GAZ:00075956</oboInOwl:id>
        <rdfs:label>Kouga Local Municipality</rdfs:label>
    </owl:NamedIndividual>
    


    <!-- http://purl.obolibrary.org/obo/GAZ_00075957 -->

    <owl:NamedIndividual rdf:about="http://purl.obolibrary.org/obo/GAZ_00075957">
        <obo:RO_0001025 rdf:resource="http://purl.obolibrary.org/obo/GAZ_00032861"/>
        <obo:IAO_0000115>A local municipality in Amatole District Municipality.</obo:IAO_0000115>
        <oboInOwl:hasOBONamespace>GAZ</oboInOwl:hasOBONamespace>
        <oboInOwl:id>GAZ:00075957</oboInOwl:id>
        <rdfs:label>Ngqushwa Local Municipality</rdfs:label>
    </owl:NamedIndividual>
    


    <!-- http://purl.obolibrary.org/obo/GAZ_00075958 -->

    <owl:NamedIndividual rdf:about="http://purl.obolibrary.org/obo/GAZ_00075958">
        <obo:RO_0001025 rdf:resource="http://purl.obolibrary.org/obo/GAZ_00032861"/>
        <obo:IAO_0000115>A municipality situated on the east coast of Eastern Cape Province, South Africa. Established 2000 after South Africa&apos;s re-organisation of municipal areas, and includes East London, Bhisho and King William&apos;s Town, as well as the large townships of Mdantsane and Zwelitsha. It is part of the Amatole District Municipality.</obo:IAO_0000115>
        <oboInOwl:hasOBONamespace>GAZ</oboInOwl:hasOBONamespace>
        <oboInOwl:id>GAZ:00075958</oboInOwl:id>
        <rdfs:label>Buffalo City Local Municipality</rdfs:label>
    </owl:NamedIndividual>
    


    <!-- http://purl.obolibrary.org/obo/GAZ_00075959 -->

    <owl:NamedIndividual rdf:about="http://purl.obolibrary.org/obo/GAZ_00075959">
        <obo:RO_0001025 rdf:resource="http://purl.obolibrary.org/obo/GAZ_00032861"/>
        <obo:IAO_0000115>A local municipality in Amatole District Municipality.</obo:IAO_0000115>
        <oboInOwl:hasOBONamespace>GAZ</oboInOwl:hasOBONamespace>
        <oboInOwl:id>GAZ:00075959</oboInOwl:id>
        <rdfs:label>Amahlathi Local Municipality</rdfs:label>
    </owl:NamedIndividual>
    


    <!-- http://purl.obolibrary.org/obo/GAZ_00075960 -->

    <owl:NamedIndividual rdf:about="http://purl.obolibrary.org/obo/GAZ_00075960">
        <obo:RO_0001025 rdf:resource="http://purl.obolibrary.org/obo/GAZ_00032861"/>
        <obo:IAO_0000115>A local municipality in Amatole District Municipality.</obo:IAO_0000115>
        <oboInOwl:hasOBONamespace>GAZ</oboInOwl:hasOBONamespace>
        <oboInOwl:id>GAZ:00075960</oboInOwl:id>
        <rdfs:label>Nkonkobe Local Municipality</rdfs:label>
    </owl:NamedIndividual>
    


    <!-- http://purl.obolibrary.org/obo/GAZ_00075961 -->

    <owl:NamedIndividual rdf:about="http://purl.obolibrary.org/obo/GAZ_00075961">
        <obo:RO_0001025 rdf:resource="http://purl.obolibrary.org/obo/GAZ_00032861"/>
        <obo:IAO_0000115>A local municipality in Amatole District Municipality.</obo:IAO_0000115>
        <oboInOwl:hasOBONamespace>GAZ</oboInOwl:hasOBONamespace>
        <oboInOwl:id>GAZ:00075961</oboInOwl:id>
        <rdfs:label>Mnquma Local Municipality</rdfs:label>
    </owl:NamedIndividual>
    


    <!-- http://purl.obolibrary.org/obo/GAZ_00075962 -->

    <owl:NamedIndividual rdf:about="http://purl.obolibrary.org/obo/GAZ_00075962">
        <obo:RO_0001025 rdf:resource="http://purl.obolibrary.org/obo/GAZ_00032861"/>
        <obo:IAO_0000115>A local municipality in Amatole District Municipality.</obo:IAO_0000115>
        <oboInOwl:hasOBONamespace>GAZ</oboInOwl:hasOBONamespace>
        <oboInOwl:id>GAZ:00075962</oboInOwl:id>
        <rdfs:label>Mbhashe Local Municipality</rdfs:label>
    </owl:NamedIndividual>
    


    <!-- http://purl.obolibrary.org/obo/GAZ_00075963 -->

    <owl:NamedIndividual rdf:about="http://purl.obolibrary.org/obo/GAZ_00075963">
        <obo:RO_0001025 rdf:resource="http://purl.obolibrary.org/obo/GAZ_00032861"/>
        <obo:IAO_0000115>A local municipality in Amatole District Municipality.</obo:IAO_0000115>
        <oboInOwl:hasOBONamespace>GAZ</oboInOwl:hasOBONamespace>
        <oboInOwl:id>GAZ:00075963</oboInOwl:id>
        <rdfs:label>Nxuba Local Municipality</rdfs:label>
    </owl:NamedIndividual>
    


    <!-- http://purl.obolibrary.org/obo/GAZ_00075964 -->

    <owl:NamedIndividual rdf:about="http://purl.obolibrary.org/obo/GAZ_00075964">
        <obo:RO_0001025 rdf:resource="http://purl.obolibrary.org/obo/GAZ_00032861"/>
        <obo:IAO_0000115>A local municipality in Amatole District Municipality.</obo:IAO_0000115>
        <oboInOwl:hasOBONamespace>GAZ</oboInOwl:hasOBONamespace>
        <oboInOwl:id>GAZ:00075964</oboInOwl:id>
        <rdfs:label>Great Kei Local Municipality</rdfs:label>
    </owl:NamedIndividual>
    


    <!-- http://purl.obolibrary.org/obo/GAZ_00075965 -->

    <owl:NamedIndividual rdf:about="http://purl.obolibrary.org/obo/GAZ_00075965">
        <obo:RO_0001025 rdf:resource="http://purl.obolibrary.org/obo/GAZ_00032857"/>
        <obo:IAO_0000115>A local municipality in Chris Hani District Municipality, Eastern Cape.</obo:IAO_0000115>
        <oboInOwl:hasOBONamespace>GAZ</oboInOwl:hasOBONamespace>
        <oboInOwl:id>GAZ:00075965</oboInOwl:id>
        <rdfs:label>Lukanji Local Municipality</rdfs:label>
    </owl:NamedIndividual>
    


    <!-- http://purl.obolibrary.org/obo/GAZ_00075966 -->

    <owl:NamedIndividual rdf:about="http://purl.obolibrary.org/obo/GAZ_00075966">
        <obo:RO_0001025 rdf:resource="http://purl.obolibrary.org/obo/GAZ_00032857"/>
        <obo:IAO_0000115>A local municipality in Chris Hani District Municipality, Eastern Cape.</obo:IAO_0000115>
        <oboInOwl:hasOBONamespace>GAZ</oboInOwl:hasOBONamespace>
        <oboInOwl:id>GAZ:00075966</oboInOwl:id>
        <rdfs:label>Inkwanca Local Municipality</rdfs:label>
    </owl:NamedIndividual>
    


    <!-- http://purl.obolibrary.org/obo/GAZ_00075967 -->

    <owl:NamedIndividual rdf:about="http://purl.obolibrary.org/obo/GAZ_00075967">
        <obo:RO_0001025 rdf:resource="http://purl.obolibrary.org/obo/GAZ_00032857"/>
        <obo:IAO_0000115>A local municipality in Chris Hani District Municipality, Eastern Cape.</obo:IAO_0000115>
        <oboInOwl:hasOBONamespace>GAZ</oboInOwl:hasOBONamespace>
        <oboInOwl:id>GAZ:00075967</oboInOwl:id>
        <rdfs:label>Sakhisizwe Local Municipality</rdfs:label>
    </owl:NamedIndividual>
    


    <!-- http://purl.obolibrary.org/obo/GAZ_00075968 -->

    <owl:NamedIndividual rdf:about="http://purl.obolibrary.org/obo/GAZ_00075968">
        <obo:RO_0001025 rdf:resource="http://purl.obolibrary.org/obo/GAZ_00032857"/>
        <obo:IAO_0000115>A local municipality in Chris Hani District Municipality, Eastern Cape.</obo:IAO_0000115>
        <oboInOwl:hasOBONamespace>GAZ</oboInOwl:hasOBONamespace>
        <oboInOwl:id>GAZ:00075968</oboInOwl:id>
        <rdfs:label>Engcobo Local Municipality</rdfs:label>
    </owl:NamedIndividual>
    


    <!-- http://purl.obolibrary.org/obo/GAZ_00075969 -->

    <owl:NamedIndividual rdf:about="http://purl.obolibrary.org/obo/GAZ_00075969">
        <obo:RO_0001025 rdf:resource="http://purl.obolibrary.org/obo/GAZ_00032857"/>
        <obo:IAO_0000115>A local municipality in Chris Hani District Municipality, Eastern Cape. The seat is Cradock.</obo:IAO_0000115>
        <oboInOwl:hasOBONamespace>GAZ</oboInOwl:hasOBONamespace>
        <oboInOwl:id>GAZ:00075969</oboInOwl:id>
        <rdfs:label>Inxuba Yethemba Local Municipality</rdfs:label>
    </owl:NamedIndividual>
    


    <!-- http://purl.obolibrary.org/obo/GAZ_00075970 -->

    <owl:NamedIndividual rdf:about="http://purl.obolibrary.org/obo/GAZ_00075970">
        <obo:RO_0001025 rdf:resource="http://purl.obolibrary.org/obo/GAZ_00032857"/>
        <obo:IAO_0000115>A local municipality in Chris Hani District Municipality, Eastern Cape.</obo:IAO_0000115>
        <oboInOwl:hasOBONamespace>GAZ</oboInOwl:hasOBONamespace>
        <oboInOwl:id>GAZ:00075970</oboInOwl:id>
        <rdfs:label>Intsika Yethu Local Municipality</rdfs:label>
    </owl:NamedIndividual>
    


    <!-- http://purl.obolibrary.org/obo/GAZ_00075971 -->

    <owl:NamedIndividual rdf:about="http://purl.obolibrary.org/obo/GAZ_00075971">
        <obo:RO_0001025 rdf:resource="http://purl.obolibrary.org/obo/GAZ_00032857"/>
        <obo:IAO_0000115>A local municipality in Chris Hani District Municipality, Eastern Cape.</obo:IAO_0000115>
        <oboInOwl:hasOBONamespace>GAZ</oboInOwl:hasOBONamespace>
        <oboInOwl:id>GAZ:00075971</oboInOwl:id>
        <rdfs:label>Emalahleni Local Municipality</rdfs:label>
    </owl:NamedIndividual>
    


    <!-- http://purl.obolibrary.org/obo/GAZ_00075972 -->

    <owl:NamedIndividual rdf:about="http://purl.obolibrary.org/obo/GAZ_00075972">
        <obo:RO_0001025 rdf:resource="http://purl.obolibrary.org/obo/GAZ_00032857"/>
        <obo:IAO_0000115>A local municipality in Chris Hani District Municipality, Eastern Cape.</obo:IAO_0000115>
        <oboInOwl:hasOBONamespace>GAZ</oboInOwl:hasOBONamespace>
        <oboInOwl:id>GAZ:00075972</oboInOwl:id>
        <rdfs:label>Tsolwana Local Municipality</rdfs:label>
    </owl:NamedIndividual>
    


    <!-- http://purl.obolibrary.org/obo/GAZ_00075973 -->

    <owl:NamedIndividual rdf:about="http://purl.obolibrary.org/obo/GAZ_00075973">
        <obo:RO_0001025 rdf:resource="http://purl.obolibrary.org/obo/GAZ_00032862"/>
        <obo:IAO_0000115>A local municipality in Ukhahlamba District Municipality.</obo:IAO_0000115>
        <oboInOwl:hasOBONamespace>GAZ</oboInOwl:hasOBONamespace>
        <oboInOwl:id>GAZ:00075973</oboInOwl:id>
        <rdfs:label>Senqu Local Municipality</rdfs:label>
    </owl:NamedIndividual>
    


    <!-- http://purl.obolibrary.org/obo/GAZ_00075974 -->

    <owl:NamedIndividual rdf:about="http://purl.obolibrary.org/obo/GAZ_00075974">
        <obo:RO_0001025 rdf:resource="http://purl.obolibrary.org/obo/GAZ_00032862"/>
        <obo:IAO_0000115>A local municipality in Ukhahlamba District Municipality.</obo:IAO_0000115>
        <oboInOwl:hasOBONamespace>GAZ</oboInOwl:hasOBONamespace>
        <oboInOwl:id>GAZ:00075974</oboInOwl:id>
        <rdfs:label>Elundini Local Municipality</rdfs:label>
    </owl:NamedIndividual>
    


    <!-- http://purl.obolibrary.org/obo/GAZ_00075975 -->

    <owl:NamedIndividual rdf:about="http://purl.obolibrary.org/obo/GAZ_00075975">
        <obo:RO_0001025 rdf:resource="http://purl.obolibrary.org/obo/GAZ_00032862"/>
        <obo:IAO_0000115>A local municipality in Ukhahlamba District Municipality.</obo:IAO_0000115>
        <oboInOwl:hasOBONamespace>GAZ</oboInOwl:hasOBONamespace>
        <oboInOwl:id>GAZ:00075975</oboInOwl:id>
        <rdfs:label>Gariep Local Municipality</rdfs:label>
    </owl:NamedIndividual>
    


    <!-- http://purl.obolibrary.org/obo/GAZ_00075976 -->

    <owl:NamedIndividual rdf:about="http://purl.obolibrary.org/obo/GAZ_00075976">
        <obo:RO_0001025 rdf:resource="http://purl.obolibrary.org/obo/GAZ_00032862"/>
        <obo:IAO_0000115>A local municipality in Ukhahlamba District Municipality.</obo:IAO_0000115>
        <oboInOwl:hasOBONamespace>GAZ</oboInOwl:hasOBONamespace>
        <oboInOwl:id>GAZ:00075976</oboInOwl:id>
        <rdfs:label>Maletswai Local Municipality</rdfs:label>
    </owl:NamedIndividual>
    


    <!-- http://purl.obolibrary.org/obo/GAZ_00075977 -->

    <owl:NamedIndividual rdf:about="http://purl.obolibrary.org/obo/GAZ_00075977">
        <obo:RO_0001025 rdf:resource="http://purl.obolibrary.org/obo/GAZ_00032860"/>
        <obo:IAO_0000115>A local municipality in OR Thambo District Municipality.</obo:IAO_0000115>
        <oboInOwl:hasOBONamespace>GAZ</oboInOwl:hasOBONamespace>
        <oboInOwl:id>GAZ:00075977</oboInOwl:id>
        <rdfs:label>Nyandeni Local Municipality</rdfs:label>
    </owl:NamedIndividual>
    


    <!-- http://purl.obolibrary.org/obo/GAZ_00075978 -->

    <owl:NamedIndividual rdf:about="http://purl.obolibrary.org/obo/GAZ_00075978">
        <obo:RO_0001025 rdf:resource="http://purl.obolibrary.org/obo/GAZ_00032860"/>
        <obo:IAO_0000115>A local municipality in OR Thambo District Municipality.</obo:IAO_0000115>
        <oboInOwl:hasOBONamespace>GAZ</oboInOwl:hasOBONamespace>
        <oboInOwl:id>GAZ:00075978</oboInOwl:id>
        <rdfs:label>Mhlontlo Local Municipality</rdfs:label>
    </owl:NamedIndividual>
    


    <!-- http://purl.obolibrary.org/obo/GAZ_00075979 -->

    <owl:NamedIndividual rdf:about="http://purl.obolibrary.org/obo/GAZ_00075979">
        <obo:RO_0001025 rdf:resource="http://purl.obolibrary.org/obo/GAZ_00032860"/>
        <obo:IAO_0000115>A local municipality in OR Thambo District Municipality.</obo:IAO_0000115>
        <oboInOwl:hasOBONamespace>GAZ</oboInOwl:hasOBONamespace>
        <oboInOwl:id>GAZ:00075979</oboInOwl:id>
        <rdfs:label>Port Saint Johns Local Municipality</rdfs:label>
    </owl:NamedIndividual>
    


    <!-- http://purl.obolibrary.org/obo/GAZ_00075980 -->

    <owl:NamedIndividual rdf:about="http://purl.obolibrary.org/obo/GAZ_00075980">
        <obo:RO_0001025 rdf:resource="http://purl.obolibrary.org/obo/GAZ_00032860"/>
        <obo:IAO_0000115>A local municipality in OR Thambo District Municipality.</obo:IAO_0000115>
        <oboInOwl:hasOBONamespace>GAZ</oboInOwl:hasOBONamespace>
        <oboInOwl:id>GAZ:00075980</oboInOwl:id>
        <rdfs:label>Ntabankulu Local Municipality</rdfs:label>
    </owl:NamedIndividual>
    


    <!-- http://purl.obolibrary.org/obo/GAZ_00075981 -->

    <owl:NamedIndividual rdf:about="http://purl.obolibrary.org/obo/GAZ_00075981">
        <obo:RO_0001025 rdf:resource="http://purl.obolibrary.org/obo/GAZ_00032860"/>
        <obo:IAO_0000115>A local municipality in OR Thambo District Municipality.</obo:IAO_0000115>
        <oboInOwl:hasOBONamespace>GAZ</oboInOwl:hasOBONamespace>
        <oboInOwl:id>GAZ:00075981</oboInOwl:id>
        <rdfs:label>King Sabata Dalindyebo Local Municipality</rdfs:label>
    </owl:NamedIndividual>
    


    <!-- http://purl.obolibrary.org/obo/GAZ_00075982 -->

    <owl:NamedIndividual rdf:about="http://purl.obolibrary.org/obo/GAZ_00075982">
        <obo:RO_0001025 rdf:resource="http://purl.obolibrary.org/obo/GAZ_00032860"/>
        <obo:IAO_0000115>A local municipality in OR Thambo District Municipality.</obo:IAO_0000115>
        <oboInOwl:hasOBONamespace>GAZ</oboInOwl:hasOBONamespace>
        <oboInOwl:id>GAZ:00075982</oboInOwl:id>
        <rdfs:label>Qaukeni Local Municipality</rdfs:label>
    </owl:NamedIndividual>
    


    <!-- http://purl.obolibrary.org/obo/GAZ_00075983 -->

    <owl:NamedIndividual rdf:about="http://purl.obolibrary.org/obo/GAZ_00075983">
        <obo:RO_0001025 rdf:resource="http://purl.obolibrary.org/obo/GAZ_00032860"/>
        <obo:IAO_0000115>A local municipality in OR Thambo District Municipality. A local municipality in OR Thambo District Municipality.</obo:IAO_0000115>
        <oboInOwl:hasOBONamespace>GAZ</oboInOwl:hasOBONamespace>
        <oboInOwl:id>GAZ:00075983</oboInOwl:id>
        <rdfs:label>Mbizana Local Municipality</rdfs:label>
    </owl:NamedIndividual>
    


    <!-- http://purl.obolibrary.org/obo/GAZ_00075984 -->

    <owl:NamedIndividual rdf:about="http://purl.obolibrary.org/obo/GAZ_00075984">
        <obo:RO_0001025 rdf:resource="http://purl.obolibrary.org/obo/GAZ_00032863"/>
        <obo:IAO_0000115>A local municipality in Alfred Nzo District Municipality.</obo:IAO_0000115>
        <oboInOwl:hasOBONamespace>GAZ</oboInOwl:hasOBONamespace>
        <oboInOwl:id>GAZ:00075984</oboInOwl:id>
        <rdfs:label>Umzimkhulu Local Municipality</rdfs:label>
    </owl:NamedIndividual>
    


    <!-- http://purl.obolibrary.org/obo/GAZ_00075985 -->

    <owl:NamedIndividual rdf:about="http://purl.obolibrary.org/obo/GAZ_00075985">
        <obo:RO_0001025 rdf:resource="http://purl.obolibrary.org/obo/GAZ_00032863"/>
        <obo:IAO_0000115>A District Management Area in Alfred Nzo District Municipality.</obo:IAO_0000115>
        <oboInOwl:hasOBONamespace>GAZ</oboInOwl:hasOBONamespace>
        <oboInOwl:id>GAZ:00075985</oboInOwl:id>
        <rdfs:label>O&apos;Conners Camp</rdfs:label>
    </owl:NamedIndividual>
    


    <!-- http://purl.obolibrary.org/obo/GAZ_00075986 -->

    <owl:NamedIndividual rdf:about="http://purl.obolibrary.org/obo/GAZ_00075986">
        <obo:RO_0001025 rdf:resource="http://purl.obolibrary.org/obo/GAZ_00032863"/>
        <obo:IAO_0000115>A local municipality in Alfred Nzo District Municipality.</obo:IAO_0000115>
        <oboInOwl:hasOBONamespace>GAZ</oboInOwl:hasOBONamespace>
        <oboInOwl:id>GAZ:00075986</oboInOwl:id>
        <rdfs:label>Umzimvubu Local Municipality</rdfs:label>
    </owl:NamedIndividual>
    


    <!-- http://purl.obolibrary.org/obo/GAZ_00075987 -->

    <owl:NamedIndividual rdf:about="http://purl.obolibrary.org/obo/GAZ_00075987">
        <obo:RO_0001025 rdf:resource="http://purl.obolibrary.org/obo/GAZ_00032866"/>
        <obo:IAO_0000115>A national park and District Management Area in Thabo Mofutsanyane District Municipality. The park is located in Free State, Republic of South Africa, near the Lesotho border.</obo:IAO_0000115>
        <oboInOwl:hasOBONamespace>GAZ</oboInOwl:hasOBONamespace>
        <oboInOwl:id>GAZ:00075987</oboInOwl:id>
        <rdfs:label>Golden Gate Highlands National Park</rdfs:label>
    </owl:NamedIndividual>
    


    <!-- http://purl.obolibrary.org/obo/GAZ_00075988 -->

    <owl:NamedIndividual rdf:about="http://purl.obolibrary.org/obo/GAZ_00075988">
        <obo:RO_0001025 rdf:resource="http://purl.obolibrary.org/obo/GAZ_00032865"/>
        <obo:IAO_0000115>A local municipality in Fezile Dabi District Municipality.</obo:IAO_0000115>
        <oboInOwl:hasOBONamespace>GAZ</oboInOwl:hasOBONamespace>
        <oboInOwl:id>GAZ:00075988</oboInOwl:id>
        <rdfs:label>Metsimaholo Local Municipality</rdfs:label>
    </owl:NamedIndividual>
    


    <!-- http://purl.obolibrary.org/obo/GAZ_00075989 -->

    <owl:NamedIndividual rdf:about="http://purl.obolibrary.org/obo/GAZ_00075989">
        <obo:RO_0001025 rdf:resource="http://purl.obolibrary.org/obo/GAZ_00032865"/>
        <obo:IAO_0000115>A local municipality in Fezile Dabi District Municipality.</obo:IAO_0000115>
        <oboInOwl:hasOBONamespace>GAZ</oboInOwl:hasOBONamespace>
        <oboInOwl:id>GAZ:00075989</oboInOwl:id>
        <rdfs:label>Moqhaka Local Municipality</rdfs:label>
    </owl:NamedIndividual>
    


    <!-- http://purl.obolibrary.org/obo/GAZ_00075990 -->

    <owl:NamedIndividual rdf:about="http://purl.obolibrary.org/obo/GAZ_00075990">
        <obo:RO_0001025 rdf:resource="http://purl.obolibrary.org/obo/GAZ_00032865"/>
        <obo:IAO_0000115>A local municipality in Fezile Dabi District Municipality.</obo:IAO_0000115>
        <oboInOwl:hasOBONamespace>GAZ</oboInOwl:hasOBONamespace>
        <oboInOwl:id>GAZ:00075990</oboInOwl:id>
        <rdfs:label>Mafube Local Municipality</rdfs:label>
    </owl:NamedIndividual>
    


    <!-- http://purl.obolibrary.org/obo/GAZ_00075991 -->

    <owl:NamedIndividual rdf:about="http://purl.obolibrary.org/obo/GAZ_00075991">
        <obo:RO_0001025 rdf:resource="http://purl.obolibrary.org/obo/GAZ_00032865"/>
        <obo:IAO_0000115>A local municipality in Fezile Dabi District Municipality.</obo:IAO_0000115>
        <oboInOwl:hasOBONamespace>GAZ</oboInOwl:hasOBONamespace>
        <oboInOwl:id>GAZ:00075991</oboInOwl:id>
        <rdfs:label>Ngwathe Local Municipality</rdfs:label>
    </owl:NamedIndividual>
    


    <!-- http://purl.obolibrary.org/obo/GAZ_00075992 -->

    <owl:NamedIndividual rdf:about="http://purl.obolibrary.org/obo/GAZ_00075992">
        <obo:RO_0001025 rdf:resource="http://purl.obolibrary.org/obo/GAZ_00032866"/>
        <obo:IAO_0000115>A local municipality in Thabo Mofutsanyane District Municipality.</obo:IAO_0000115>
        <oboInOwl:hasOBONamespace>GAZ</oboInOwl:hasOBONamespace>
        <oboInOwl:id>GAZ:00075992</oboInOwl:id>
        <rdfs:label>Nketoana Local Municipality</rdfs:label>
    </owl:NamedIndividual>
    


    <!-- http://purl.obolibrary.org/obo/GAZ_00075993 -->

    <owl:NamedIndividual rdf:about="http://purl.obolibrary.org/obo/GAZ_00075993">
        <obo:RO_0001025 rdf:resource="http://purl.obolibrary.org/obo/GAZ_00032866"/>
        <obo:IAO_0000115>A local municipality in Thabo Mofutsanyane District Municipality.</obo:IAO_0000115>
        <oboInOwl:hasOBONamespace>GAZ</oboInOwl:hasOBONamespace>
        <oboInOwl:id>GAZ:00075993</oboInOwl:id>
        <rdfs:label>Phumelela Local Municipality</rdfs:label>
    </owl:NamedIndividual>
    


    <!-- http://purl.obolibrary.org/obo/GAZ_00075994 -->

    <owl:NamedIndividual rdf:about="http://purl.obolibrary.org/obo/GAZ_00075994">
        <obo:RO_0001025 rdf:resource="http://purl.obolibrary.org/obo/GAZ_00032866"/>
        <obo:IAO_0000115>A local municipality in Thabo Mofutsanyane District Municipality.</obo:IAO_0000115>
        <oboInOwl:hasOBONamespace>GAZ</oboInOwl:hasOBONamespace>
        <oboInOwl:id>GAZ:00075994</oboInOwl:id>
        <rdfs:label>Dihlabeng Local Municipality</rdfs:label>
    </owl:NamedIndividual>
    


    <!-- http://purl.obolibrary.org/obo/GAZ_00075995 -->

    <owl:NamedIndividual rdf:about="http://purl.obolibrary.org/obo/GAZ_00075995">
        <obo:RO_0001025 rdf:resource="http://purl.obolibrary.org/obo/GAZ_00032866"/>
        <obo:IAO_0000115>A local municipality in Thabo Mofutsanyane District Municipality.</obo:IAO_0000115>
        <oboInOwl:hasOBONamespace>GAZ</oboInOwl:hasOBONamespace>
        <oboInOwl:id>GAZ:00075995</oboInOwl:id>
        <rdfs:label>Maluti a Phofung Local Municipality</rdfs:label>
    </owl:NamedIndividual>
    


    <!-- http://purl.obolibrary.org/obo/GAZ_00075996 -->

    <owl:NamedIndividual rdf:about="http://purl.obolibrary.org/obo/GAZ_00075996">
        <obo:RO_0001025 rdf:resource="http://purl.obolibrary.org/obo/GAZ_00032866"/>
        <obo:IAO_0000115>A local municipality in Thabo Mofutsanyane District Municipality.</obo:IAO_0000115>
        <oboInOwl:hasOBONamespace>GAZ</oboInOwl:hasOBONamespace>
        <oboInOwl:id>GAZ:00075996</oboInOwl:id>
        <rdfs:label>Setsoto Local Municipality</rdfs:label>
    </owl:NamedIndividual>
    


    <!-- http://purl.obolibrary.org/obo/GAZ_00075997 -->

    <owl:NamedIndividual rdf:about="http://purl.obolibrary.org/obo/GAZ_00075997">
        <obo:RO_0001025 rdf:resource="http://purl.obolibrary.org/obo/GAZ_00032867"/>
        <obo:IAO_0000115>A local municipality in Lejweleputswa District Municipality.</obo:IAO_0000115>
        <oboInOwl:hasOBONamespace>GAZ</oboInOwl:hasOBONamespace>
        <oboInOwl:id>GAZ:00075997</oboInOwl:id>
        <rdfs:label>Masilonyana Local Municipality</rdfs:label>
    </owl:NamedIndividual>
    


    <!-- http://purl.obolibrary.org/obo/GAZ_00075998 -->

    <owl:NamedIndividual rdf:about="http://purl.obolibrary.org/obo/GAZ_00075998">
        <obo:RO_0001025 rdf:resource="http://purl.obolibrary.org/obo/GAZ_00032867"/>
        <obo:IAO_0000115>A local municipality in Lejweleputswa District Municipality.</obo:IAO_0000115>
        <oboInOwl:hasOBONamespace>GAZ</oboInOwl:hasOBONamespace>
        <oboInOwl:id>GAZ:00075998</oboInOwl:id>
        <rdfs:label>Nala Local Municipality</rdfs:label>
    </owl:NamedIndividual>
    


    <!-- http://purl.obolibrary.org/obo/GAZ_00075999 -->

    <owl:NamedIndividual rdf:about="http://purl.obolibrary.org/obo/GAZ_00075999">
        <obo:RO_0001025 rdf:resource="http://purl.obolibrary.org/obo/GAZ_00032867"/>
        <obo:IAO_0000115>A local municipality in Lejweleputswa District Municipality.</obo:IAO_0000115>
        <oboInOwl:hasOBONamespace>GAZ</oboInOwl:hasOBONamespace>
        <oboInOwl:id>GAZ:00075999</oboInOwl:id>
        <rdfs:label>Tswelopele Local Municipality</rdfs:label>
    </owl:NamedIndividual>
    


    <!-- http://purl.obolibrary.org/obo/GAZ_00076000 -->

    <owl:NamedIndividual rdf:about="http://purl.obolibrary.org/obo/GAZ_00076000">
        <obo:RO_0001025 rdf:resource="http://purl.obolibrary.org/obo/GAZ_00032867"/>
        <obo:IAO_0000115>A local municipality in Lejweleputswa District Municipality.</obo:IAO_0000115>
        <oboInOwl:hasOBONamespace>GAZ</oboInOwl:hasOBONamespace>
        <oboInOwl:id>GAZ:00076000</oboInOwl:id>
        <rdfs:label>Tokologo Local Municipality</rdfs:label>
    </owl:NamedIndividual>
    


    <!-- http://purl.obolibrary.org/obo/GAZ_00076001 -->

    <owl:NamedIndividual rdf:about="http://purl.obolibrary.org/obo/GAZ_00076001">
        <obo:RO_0001025 rdf:resource="http://purl.obolibrary.org/obo/GAZ_00032867"/>
        <obo:IAO_0000115>A local municipality in Lejweleputswa District Municipality.</obo:IAO_0000115>
        <oboInOwl:hasOBONamespace>GAZ</oboInOwl:hasOBONamespace>
        <oboInOwl:id>GAZ:00076001</oboInOwl:id>
        <rdfs:label>Matjhabeng Local Municipality</rdfs:label>
    </owl:NamedIndividual>
    


    <!-- http://purl.obolibrary.org/obo/GAZ_00076002 -->

    <owl:NamedIndividual rdf:about="http://purl.obolibrary.org/obo/GAZ_00076002">
        <obo:RO_0001025 rdf:resource="http://purl.obolibrary.org/obo/GAZ_00032868"/>
        <obo:IAO_0000115>A local municipality in Motheo District Municipality.</obo:IAO_0000115>
        <oboInOwl:hasOBONamespace>GAZ</oboInOwl:hasOBONamespace>
        <oboInOwl:id>GAZ:00076002</oboInOwl:id>
        <rdfs:label>Naledi Local Municipality</rdfs:label>
    </owl:NamedIndividual>
    


    <!-- http://purl.obolibrary.org/obo/GAZ_00076003 -->

    <owl:NamedIndividual rdf:about="http://purl.obolibrary.org/obo/GAZ_00076003">
        <obo:RO_0001025 rdf:resource="http://purl.obolibrary.org/obo/GAZ_00032868"/>
        <obo:IAO_0000115>A local municipality in Motheo District Municipality.</obo:IAO_0000115>
        <oboInOwl:hasOBONamespace>GAZ</oboInOwl:hasOBONamespace>
        <oboInOwl:id>GAZ:00076003</oboInOwl:id>
        <rdfs:label>Mangaung Local Municipality</rdfs:label>
    </owl:NamedIndividual>
    


    <!-- http://purl.obolibrary.org/obo/GAZ_00076004 -->

    <owl:NamedIndividual rdf:about="http://purl.obolibrary.org/obo/GAZ_00076004">
        <obo:RO_0001025 rdf:resource="http://purl.obolibrary.org/obo/GAZ_00032868"/>
        <obo:IAO_0000115>A local municipality in Motheo District Municipality.</obo:IAO_0000115>
        <oboInOwl:hasOBONamespace>GAZ</oboInOwl:hasOBONamespace>
        <oboInOwl:id>GAZ:00076004</oboInOwl:id>
        <rdfs:label>Mantsopa Local Municipality</rdfs:label>
    </owl:NamedIndividual>
    


    <!-- http://purl.obolibrary.org/obo/GAZ_00076005 -->

    <owl:NamedIndividual rdf:about="http://purl.obolibrary.org/obo/GAZ_00076005">
        <obo:RO_0001025 rdf:resource="http://purl.obolibrary.org/obo/GAZ_00032864"/>
        <obo:IAO_0000115>A local municipality located in the southern Free State Province in Xhariep District Municipality.</obo:IAO_0000115>
        <oboInOwl:hasOBONamespace>GAZ</oboInOwl:hasOBONamespace>
        <oboInOwl:id>GAZ:00076005</oboInOwl:id>
        <rdfs:label>Kopanong Local Municipality</rdfs:label>
    </owl:NamedIndividual>
    


    <!-- http://purl.obolibrary.org/obo/GAZ_00076006 -->

    <owl:NamedIndividual rdf:about="http://purl.obolibrary.org/obo/GAZ_00076006">
        <obo:RO_0001025 rdf:resource="http://purl.obolibrary.org/obo/GAZ_00032864"/>
        <obo:IAO_0000115>A local municipality located in the south-western Free State in Xhariep District Municipality.</obo:IAO_0000115>
        <oboInOwl:hasOBONamespace>GAZ</oboInOwl:hasOBONamespace>
        <oboInOwl:id>GAZ:00076006</oboInOwl:id>
        <rdfs:label>Letsemeng Local Municipality</rdfs:label>
    </owl:NamedIndividual>
    


    <!-- http://purl.obolibrary.org/obo/GAZ_00076007 -->

    <owl:NamedIndividual rdf:about="http://purl.obolibrary.org/obo/GAZ_00076007">
        <obo:RO_0001025 rdf:resource="http://purl.obolibrary.org/obo/GAZ_00032864"/>
        <obo:IAO_0000115>A local municipality located in the south-eastern Free State in Xhariep District Municipality.</obo:IAO_0000115>
        <oboInOwl:hasOBONamespace>GAZ</oboInOwl:hasOBONamespace>
        <oboInOwl:id>GAZ:00076007</oboInOwl:id>
        <rdfs:label>Mohokare Local Municipality</rdfs:label>
    </owl:NamedIndividual>
    


    <!-- http://purl.obolibrary.org/obo/GAZ_00076008 -->

    <owl:NamedIndividual rdf:about="http://purl.obolibrary.org/obo/GAZ_00076008">
        <obo:RO_0001025 rdf:resource="http://purl.obolibrary.org/obo/GAZ_00032862"/>
        <obo:IAO_0000115>A nature reserve and District Management Area in Ukhahlamba District Municipality.</obo:IAO_0000115>
        <oboInOwl:hasOBONamespace>GAZ</oboInOwl:hasOBONamespace>
        <oboInOwl:id>GAZ:00076008</oboInOwl:id>
        <rdfs:label>Oviston Nature Reserve</rdfs:label>
    </owl:NamedIndividual>
    


    <!-- http://purl.obolibrary.org/obo/GAZ_00076009 -->

    <owl:NamedIndividual rdf:about="http://purl.obolibrary.org/obo/GAZ_00076009">
        <obo:RO_0001025 rdf:resource="http://purl.obolibrary.org/obo/GAZ_00032879"/>
        <obo:IAO_0000115>A local municipality in Sedibeng District Municipality.</obo:IAO_0000115>
        <oboInOwl:hasOBONamespace>GAZ</oboInOwl:hasOBONamespace>
        <oboInOwl:id>GAZ:00076009</oboInOwl:id>
        <rdfs:label>Emfuleni Local Municipality</rdfs:label>
    </owl:NamedIndividual>
    


    <!-- http://purl.obolibrary.org/obo/GAZ_00076010 -->

    <owl:NamedIndividual rdf:about="http://purl.obolibrary.org/obo/GAZ_00076010">
        <obo:RO_0001025 rdf:resource="http://purl.obolibrary.org/obo/GAZ_00032879"/>
        <obo:IAO_0000115>A local municipality in Sedibeng District Municipality.</obo:IAO_0000115>
        <oboInOwl:hasOBONamespace>GAZ</oboInOwl:hasOBONamespace>
        <oboInOwl:id>GAZ:00076010</oboInOwl:id>
        <rdfs:label>Midvaal Local Municipality</rdfs:label>
    </owl:NamedIndividual>
    


    <!-- http://purl.obolibrary.org/obo/GAZ_00076011 -->

    <owl:NamedIndividual rdf:about="http://purl.obolibrary.org/obo/GAZ_00076011">
        <obo:RO_0001025 rdf:resource="http://purl.obolibrary.org/obo/GAZ_00032879"/>
        <obo:IAO_0000115>A local municipality in Sedibeng District Municipality.</obo:IAO_0000115>
        <oboInOwl:hasOBONamespace>GAZ</oboInOwl:hasOBONamespace>
        <oboInOwl:id>GAZ:00076011</oboInOwl:id>
        <rdfs:label>Lesedi Local Municipality</rdfs:label>
    </owl:NamedIndividual>
    


    <!-- http://purl.obolibrary.org/obo/GAZ_00076012 -->

    <owl:NamedIndividual rdf:about="http://purl.obolibrary.org/obo/GAZ_00076012">
        <obo:RO_0001025 rdf:resource="http://purl.obolibrary.org/obo/GAZ_00032880"/>
        <obo:IAO_0000115>A local municipality in Metsweding District Municipality.</obo:IAO_0000115>
        <oboInOwl:hasOBONamespace>GAZ</oboInOwl:hasOBONamespace>
        <oboInOwl:id>GAZ:00076012</oboInOwl:id>
        <rdfs:label>Nokeng tsa Taemane Local Municipality</rdfs:label>
    </owl:NamedIndividual>
    


    <!-- http://purl.obolibrary.org/obo/GAZ_00076013 -->

    <owl:NamedIndividual rdf:about="http://purl.obolibrary.org/obo/GAZ_00076013">
        <obo:RO_0001025 rdf:resource="http://purl.obolibrary.org/obo/GAZ_00032880"/>
        <obo:IAO_0000115>A local municipality in Metsweding District Municipality.</obo:IAO_0000115>
        <oboInOwl:hasOBONamespace>GAZ</oboInOwl:hasOBONamespace>
        <oboInOwl:id>GAZ:00076013</oboInOwl:id>
        <rdfs:label>Kungwini Local Municipality</rdfs:label>
    </owl:NamedIndividual>
    


    <!-- http://purl.obolibrary.org/obo/GAZ_00076014 -->

    <owl:NamedIndividual rdf:about="http://purl.obolibrary.org/obo/GAZ_00076014">
        <obo:RO_0001025 rdf:resource="http://purl.obolibrary.org/obo/GAZ_00012785"/>
        <obo:IAO_0000115>A local municipality in West Rand District Municipality, Gauteng, in South Africa.</obo:IAO_0000115>
        <oboInOwl:hasOBONamespace>GAZ</oboInOwl:hasOBONamespace>
        <oboInOwl:id>GAZ:00076014</oboInOwl:id>
        <rdfs:label>Randfontein Local Municipality</rdfs:label>
    </owl:NamedIndividual>
    


    <!-- http://purl.obolibrary.org/obo/GAZ_00076015 -->

    <owl:NamedIndividual rdf:about="http://purl.obolibrary.org/obo/GAZ_00076015">
        <obo:RO_0001025 rdf:resource="http://purl.obolibrary.org/obo/GAZ_00012785"/>
        <obo:IAO_0000115>A local municipality in West Rand District Municipality, Gauteng, in South Africa.</obo:IAO_0000115>
        <oboInOwl:hasOBONamespace>GAZ</oboInOwl:hasOBONamespace>
        <oboInOwl:id>GAZ:00076015</oboInOwl:id>
        <rdfs:label>Westonaria Local Municipality</rdfs:label>
    </owl:NamedIndividual>
    


    <!-- http://purl.obolibrary.org/obo/GAZ_00076016 -->

    <owl:NamedIndividual rdf:about="http://purl.obolibrary.org/obo/GAZ_00076016">
        <obo:RO_0001025 rdf:resource="http://purl.obolibrary.org/obo/GAZ_00012785"/>
        <obo:IAO_0000115>A local municipality in West Rand District Municipality, Gauteng, in South Africa.</obo:IAO_0000115>
        <oboInOwl:hasOBONamespace>GAZ</oboInOwl:hasOBONamespace>
        <oboInOwl:id>GAZ:00076016</oboInOwl:id>
        <rdfs:label>Mogale City Local Municipality</rdfs:label>
    </owl:NamedIndividual>
    


    <!-- http://purl.obolibrary.org/obo/GAZ_00076017 -->

    <owl:NamedIndividual rdf:about="http://purl.obolibrary.org/obo/GAZ_00076017">
        <obo:RO_0001025 rdf:resource="http://purl.obolibrary.org/obo/GAZ_00002815"/>
        <obo:IAO_0000115>A low, sedimentary range of hills, at an elevation of 1700-1800 m above sea-level, which runs in an east-west direction through Gauteng in South Africa. It forms a continental divide with run-off to the north draining into the Limpopo River and Indian Ocean and to the south draining into the Orange River and Atlantic. The Witwatersrand lies within the province of Gauteng, formerly called the PWV area, an acronym for Pretoria, Witwatersrand, and Vereeniging.</obo:IAO_0000115>
        <oboInOwl:hasOBONamespace>GAZ</oboInOwl:hasOBONamespace>
        <oboInOwl:id>GAZ:00076017</oboInOwl:id>
        <rdfs:label>Witwatersrand</rdfs:label>
    </owl:NamedIndividual>
    


    <!-- http://purl.obolibrary.org/obo/GAZ_00076018 -->

    <owl:NamedIndividual rdf:about="http://purl.obolibrary.org/obo/GAZ_00076018">
        <obo:RO_0001025 rdf:resource="http://purl.obolibrary.org/obo/GAZ_00032883"/>
        <obo:IAO_0000115>A local municipality in Mopani District Municipality.</obo:IAO_0000115>
        <oboInOwl:hasOBONamespace>GAZ</oboInOwl:hasOBONamespace>
        <oboInOwl:id>GAZ:00076018</oboInOwl:id>
        <rdfs:label>Greater Tzaneen Local Municipality</rdfs:label>
    </owl:NamedIndividual>
    


    <!-- http://purl.obolibrary.org/obo/GAZ_00076019 -->

    <owl:NamedIndividual rdf:about="http://purl.obolibrary.org/obo/GAZ_00076019">
        <obo:RO_0001025 rdf:resource="http://purl.obolibrary.org/obo/GAZ_00032883"/>
        <obo:IAO_0000115>A local municipality in Mopani District Municipality.</obo:IAO_0000115>
        <oboInOwl:hasOBONamespace>GAZ</oboInOwl:hasOBONamespace>
        <oboInOwl:id>GAZ:00076019</oboInOwl:id>
        <rdfs:label>Greater Giyani Local Municipality</rdfs:label>
    </owl:NamedIndividual>
    


    <!-- http://purl.obolibrary.org/obo/GAZ_00076020 -->

    <owl:NamedIndividual rdf:about="http://purl.obolibrary.org/obo/GAZ_00076020">
        <obo:RO_0001025 rdf:resource="http://purl.obolibrary.org/obo/GAZ_00032883"/>
        <obo:IAO_0000115>A local municipality in Mopani District Municipality.</obo:IAO_0000115>
        <oboInOwl:hasOBONamespace>GAZ</oboInOwl:hasOBONamespace>
        <oboInOwl:id>GAZ:00076020</oboInOwl:id>
        <rdfs:label>Greater Letaba Local Municipality</rdfs:label>
    </owl:NamedIndividual>
    


    <!-- http://purl.obolibrary.org/obo/GAZ_00076021 -->

    <owl:NamedIndividual rdf:about="http://purl.obolibrary.org/obo/GAZ_00076021">
        <obo:RO_0001025 rdf:resource="http://purl.obolibrary.org/obo/GAZ_00032883"/>
        <obo:IAO_0000115>A local municipality in Mopani District Municipality.</obo:IAO_0000115>
        <oboInOwl:hasOBONamespace>GAZ</oboInOwl:hasOBONamespace>
        <oboInOwl:id>GAZ:00076021</oboInOwl:id>
        <rdfs:label>Maruleng Local Municipality</rdfs:label>
    </owl:NamedIndividual>
    


    <!-- http://purl.obolibrary.org/obo/GAZ_00076022 -->

    <owl:NamedIndividual rdf:about="http://purl.obolibrary.org/obo/GAZ_00076022">
        <obo:RO_0001025 rdf:resource="http://purl.obolibrary.org/obo/GAZ_00032883"/>
        <obo:IAO_0000115>A local municipality in Mopani District Municipality.</obo:IAO_0000115>
        <oboInOwl:hasOBONamespace>GAZ</oboInOwl:hasOBONamespace>
        <oboInOwl:id>GAZ:00076022</oboInOwl:id>
        <rdfs:label>Ba-Phalaborwa Local Municipality</rdfs:label>
    </owl:NamedIndividual>
    


    <!-- http://purl.obolibrary.org/obo/GAZ_00076023 -->

    <owl:NamedIndividual rdf:about="http://purl.obolibrary.org/obo/GAZ_00076023">
        <obo:RO_0001025 rdf:resource="http://purl.obolibrary.org/obo/GAZ_00032882"/>
        <obo:IAO_0000115>A local municipality in Vhembe District Municipality.</obo:IAO_0000115>
        <oboInOwl:hasOBONamespace>GAZ</oboInOwl:hasOBONamespace>
        <oboInOwl:id>GAZ:00076023</oboInOwl:id>
        <rdfs:label>Mutale Local Municipality</rdfs:label>
    </owl:NamedIndividual>
    


    <!-- http://purl.obolibrary.org/obo/GAZ_00076024 -->

    <owl:NamedIndividual rdf:about="http://purl.obolibrary.org/obo/GAZ_00076024">
        <obo:RO_0001025 rdf:resource="http://purl.obolibrary.org/obo/GAZ_00032882"/>
        <obo:IAO_0000115>A local municipality in Vhembe District Municipality.</obo:IAO_0000115>
        <oboInOwl:hasOBONamespace>GAZ</oboInOwl:hasOBONamespace>
        <oboInOwl:id>GAZ:00076024</oboInOwl:id>
        <rdfs:label>Musina Local Municipality</rdfs:label>
    </owl:NamedIndividual>
    


    <!-- http://purl.obolibrary.org/obo/GAZ_00076025 -->

    <owl:NamedIndividual rdf:about="http://purl.obolibrary.org/obo/GAZ_00076025">
        <obo:RO_0001025 rdf:resource="http://purl.obolibrary.org/obo/GAZ_00032882"/>
        <obo:IAO_0000115>A local municipality in Vhembe District Municipality.</obo:IAO_0000115>
        <oboInOwl:hasOBONamespace>GAZ</oboInOwl:hasOBONamespace>
        <oboInOwl:id>GAZ:00076025</oboInOwl:id>
        <rdfs:label>Makhado Local Municipality</rdfs:label>
    </owl:NamedIndividual>
    


    <!-- http://purl.obolibrary.org/obo/GAZ_00076026 -->

    <owl:NamedIndividual rdf:about="http://purl.obolibrary.org/obo/GAZ_00076026">
        <obo:RO_0001025 rdf:resource="http://purl.obolibrary.org/obo/GAZ_00032882"/>
        <obo:IAO_0000115>A local municipality in Vhembe District Municipality.</obo:IAO_0000115>
        <oboInOwl:hasOBONamespace>GAZ</oboInOwl:hasOBONamespace>
        <oboInOwl:id>GAZ:00076026</oboInOwl:id>
        <rdfs:label>Thulamela Local Municipality</rdfs:label>
    </owl:NamedIndividual>
    


    <!-- http://purl.obolibrary.org/obo/GAZ_00076027 -->

    <owl:NamedIndividual rdf:about="http://purl.obolibrary.org/obo/GAZ_00076027">
        <obo:RO_0001025 rdf:resource="http://purl.obolibrary.org/obo/GAZ_00032884"/>
        <obo:IAO_0000115>A local municipality in Capricorn District Municipality.</obo:IAO_0000115>
        <oboInOwl:hasOBONamespace>GAZ</oboInOwl:hasOBONamespace>
        <oboInOwl:id>GAZ:00076027</oboInOwl:id>
        <rdfs:label>Aganang Local Municipality</rdfs:label>
    </owl:NamedIndividual>
    


    <!-- http://purl.obolibrary.org/obo/GAZ_00076028 -->

    <owl:NamedIndividual rdf:about="http://purl.obolibrary.org/obo/GAZ_00076028">
        <rdf:type rdf:resource="http://purl.obolibrary.org/obo/ENVO_00000856"/>
        <obo:RO_0001025 rdf:resource="http://purl.obolibrary.org/obo/GAZ_00032884"/>
        <obo:IAO_0000115>A municipality and the capital of the Limpopo province in South Africa.</obo:IAO_0000115>
        <oboInOwl:hasOBONamespace>GAZ</oboInOwl:hasOBONamespace>
        <oboInOwl:id>GAZ:00076028</oboInOwl:id>
        <rdfs:label>Polokwane Local Municipality</rdfs:label>
    </owl:NamedIndividual>
    


    <!-- http://purl.obolibrary.org/obo/GAZ_00076029 -->

    <owl:NamedIndividual rdf:about="http://purl.obolibrary.org/obo/GAZ_00076029">
        <obo:RO_0001025 rdf:resource="http://purl.obolibrary.org/obo/GAZ_00032884"/>
        <obo:IAO_0000115>A local municipality in Capricorn District Municipality.</obo:IAO_0000115>
        <oboInOwl:hasOBONamespace>GAZ</oboInOwl:hasOBONamespace>
        <oboInOwl:id>GAZ:00076029</oboInOwl:id>
        <rdfs:label>Lepele-Nkumpi Local Municipality</rdfs:label>
    </owl:NamedIndividual>
    


    <!-- http://purl.obolibrary.org/obo/GAZ_00076030 -->

    <owl:NamedIndividual rdf:about="http://purl.obolibrary.org/obo/GAZ_00076030">
        <obo:RO_0001025 rdf:resource="http://purl.obolibrary.org/obo/GAZ_00032884"/>
        <obo:IAO_0000115>A local municipality in Capricorn District Municipality.</obo:IAO_0000115>
        <oboInOwl:hasOBONamespace>GAZ</oboInOwl:hasOBONamespace>
        <oboInOwl:id>GAZ:00076030</oboInOwl:id>
        <rdfs:label>Molemole Local Municipality</rdfs:label>
    </owl:NamedIndividual>
    


    <!-- http://purl.obolibrary.org/obo/GAZ_00076031 -->

    <owl:NamedIndividual rdf:about="http://purl.obolibrary.org/obo/GAZ_00076031">
        <obo:RO_0001025 rdf:resource="http://purl.obolibrary.org/obo/GAZ_00032884"/>
        <obo:IAO_0000115>A local municipality in Capricorn District Municipality.</obo:IAO_0000115>
        <oboInOwl:hasOBONamespace>GAZ</oboInOwl:hasOBONamespace>
        <oboInOwl:id>GAZ:00076031</oboInOwl:id>
        <rdfs:label>Blouberg Local Municipality</rdfs:label>
    </owl:NamedIndividual>
    


    <!-- http://purl.obolibrary.org/obo/GAZ_00076032 -->

    <owl:NamedIndividual rdf:about="http://purl.obolibrary.org/obo/GAZ_00076032">
        <obo:RO_0001025 rdf:resource="http://purl.obolibrary.org/obo/GAZ_00032884"/>
        <obo:IAO_0000115>A protected area.</obo:IAO_0000115>
        <oboInOwl:hasOBONamespace>GAZ</oboInOwl:hasOBONamespace>
        <oboInOwl:id>GAZ:00076032</oboInOwl:id>
        <rdfs:label>Schuinsdraai Nature Reserve</rdfs:label>
    </owl:NamedIndividual>
    


    <!-- http://purl.obolibrary.org/obo/GAZ_00076033 -->

    <owl:NamedIndividual rdf:about="http://purl.obolibrary.org/obo/GAZ_00076033">
        <obo:RO_0001025 rdf:resource="http://purl.obolibrary.org/obo/GAZ_00012788"/>
        <obo:IAO_0000115>A local municipality in Sekhukhune District Municipality.</obo:IAO_0000115>
        <oboInOwl:hasOBONamespace>GAZ</oboInOwl:hasOBONamespace>
        <oboInOwl:id>GAZ:00076033</oboInOwl:id>
        <rdfs:label>Makhuduthamaga Local Municipality</rdfs:label>
    </owl:NamedIndividual>
    


    <!-- http://purl.obolibrary.org/obo/GAZ_00076034 -->

    <owl:NamedIndividual rdf:about="http://purl.obolibrary.org/obo/GAZ_00076034">
        <obo:RO_0001025 rdf:resource="http://purl.obolibrary.org/obo/GAZ_00012788"/>
        <obo:IAO_0000115>A local municipality in Sekhukhune District Municipality.</obo:IAO_0000115>
        <oboInOwl:hasOBONamespace>GAZ</oboInOwl:hasOBONamespace>
        <oboInOwl:id>GAZ:00076034</oboInOwl:id>
        <rdfs:label>Greater Tubatse Local Municipality</rdfs:label>
    </owl:NamedIndividual>
    


    <!-- http://purl.obolibrary.org/obo/GAZ_00076035 -->

    <owl:NamedIndividual rdf:about="http://purl.obolibrary.org/obo/GAZ_00076035">
        <obo:RO_0001025 rdf:resource="http://purl.obolibrary.org/obo/GAZ_00012788"/>
        <obo:IAO_0000115>A local municipality in Sekhukhune District Municipality.</obo:IAO_0000115>
        <oboInOwl:hasOBONamespace>GAZ</oboInOwl:hasOBONamespace>
        <oboInOwl:id>GAZ:00076035</oboInOwl:id>
        <rdfs:label>Greater Groblersdal Local Municipality</rdfs:label>
    </owl:NamedIndividual>
    


    <!-- http://purl.obolibrary.org/obo/GAZ_00076036 -->

    <owl:NamedIndividual rdf:about="http://purl.obolibrary.org/obo/GAZ_00076036">
        <obo:RO_0001025 rdf:resource="http://purl.obolibrary.org/obo/GAZ_00012788"/>
        <obo:IAO_0000115>A local municipality in Sekhukhune District Municipality.</obo:IAO_0000115>
        <oboInOwl:hasOBONamespace>GAZ</oboInOwl:hasOBONamespace>
        <oboInOwl:id>GAZ:00076036</oboInOwl:id>
        <rdfs:label>Fetakgomo Local Municipality</rdfs:label>
    </owl:NamedIndividual>
    


    <!-- http://purl.obolibrary.org/obo/GAZ_00076037 -->

    <owl:NamedIndividual rdf:about="http://purl.obolibrary.org/obo/GAZ_00076037">
        <obo:RO_0001025 rdf:resource="http://purl.obolibrary.org/obo/GAZ_00012788"/>
        <obo:IAO_0000115>A local municipality in Sekhukhune District Municipality.</obo:IAO_0000115>
        <oboInOwl:hasOBONamespace>GAZ</oboInOwl:hasOBONamespace>
        <oboInOwl:id>GAZ:00076037</oboInOwl:id>
        <rdfs:label>Greater Marble Hall Local Municipality</rdfs:label>
    </owl:NamedIndividual>
    


    <!-- http://purl.obolibrary.org/obo/GAZ_00076038 -->

    <owl:NamedIndividual rdf:about="http://purl.obolibrary.org/obo/GAZ_00076038">
        <obo:RO_0001025 rdf:resource="http://purl.obolibrary.org/obo/GAZ_00032881"/>
        <obo:IAO_0000115>A local municipality in Waterberg District Municipality.</obo:IAO_0000115>
        <oboInOwl:hasOBONamespace>GAZ</oboInOwl:hasOBONamespace>
        <oboInOwl:id>GAZ:00076038</oboInOwl:id>
        <rdfs:label>Modimolle Local Municipality</rdfs:label>
    </owl:NamedIndividual>
    


    <!-- http://purl.obolibrary.org/obo/GAZ_00076039 -->

    <owl:NamedIndividual rdf:about="http://purl.obolibrary.org/obo/GAZ_00076039">
        <obo:RO_0001025 rdf:resource="http://purl.obolibrary.org/obo/GAZ_00032881"/>
        <obo:IAO_0000115>A local municipality in Waterberg District Municipality.</obo:IAO_0000115>
        <oboInOwl:hasOBONamespace>GAZ</oboInOwl:hasOBONamespace>
        <oboInOwl:id>GAZ:00076039</oboInOwl:id>
        <rdfs:label>Mogalakwena Local Municipality</rdfs:label>
    </owl:NamedIndividual>
    


    <!-- http://purl.obolibrary.org/obo/GAZ_00076040 -->

    <owl:NamedIndividual rdf:about="http://purl.obolibrary.org/obo/GAZ_00076040">
        <obo:RO_0001025 rdf:resource="http://purl.obolibrary.org/obo/GAZ_00032881"/>
        <obo:IAO_0000115>A local municipality in Waterberg District Municipality.</obo:IAO_0000115>
        <oboInOwl:hasOBONamespace>GAZ</oboInOwl:hasOBONamespace>
        <oboInOwl:id>GAZ:00076040</oboInOwl:id>
        <rdfs:label>Thabazimbi Local Municipality</rdfs:label>
    </owl:NamedIndividual>
    


    <!-- http://purl.obolibrary.org/obo/GAZ_00076041 -->

    <owl:NamedIndividual rdf:about="http://purl.obolibrary.org/obo/GAZ_00076041">
        <obo:RO_0001025 rdf:resource="http://purl.obolibrary.org/obo/GAZ_00032881"/>
        <obo:IAO_0000115>A local municipality in Waterberg District Municipality.</obo:IAO_0000115>
        <oboInOwl:hasOBONamespace>GAZ</oboInOwl:hasOBONamespace>
        <oboInOwl:id>GAZ:00076041</oboInOwl:id>
        <rdfs:label>Lephalale Local Municipality</rdfs:label>
    </owl:NamedIndividual>
    


    <!-- http://purl.obolibrary.org/obo/GAZ_00076042 -->

    <owl:NamedIndividual rdf:about="http://purl.obolibrary.org/obo/GAZ_00076042">
        <obo:RO_0001025 rdf:resource="http://purl.obolibrary.org/obo/GAZ_00032881"/>
        <obo:IAO_0000115>A local municipality in Waterberg District Municipality.</obo:IAO_0000115>
        <oboInOwl:hasOBONamespace>GAZ</oboInOwl:hasOBONamespace>
        <oboInOwl:id>GAZ:00076042</oboInOwl:id>
        <rdfs:label>Bela-Bela Local Municipality</rdfs:label>
    </owl:NamedIndividual>
    


    <!-- http://purl.obolibrary.org/obo/GAZ_00076043 -->

    <owl:NamedIndividual rdf:about="http://purl.obolibrary.org/obo/GAZ_00076043">
        <obo:RO_0001025 rdf:resource="http://purl.obolibrary.org/obo/GAZ_00032881"/>
        <obo:IAO_0000115>A local municipality in Waterberg District Municipality.</obo:IAO_0000115>
        <oboInOwl:hasOBONamespace>GAZ</oboInOwl:hasOBONamespace>
        <oboInOwl:id>GAZ:00076043</oboInOwl:id>
        <rdfs:label>Mookgopong Local Municipality</rdfs:label>
    </owl:NamedIndividual>
    


    <!-- http://purl.obolibrary.org/obo/GAZ_00076044 -->

    <owl:NamedIndividual rdf:about="http://purl.obolibrary.org/obo/GAZ_00076044">
        <obo:RO_0001025 rdf:resource="http://purl.obolibrary.org/obo/GAZ_00032885"/>
        <obo:IAO_0000115>A local municipality in Gert Sibande District Municipality.</obo:IAO_0000115>
        <oboInOwl:hasOBONamespace>GAZ</oboInOwl:hasOBONamespace>
        <oboInOwl:id>GAZ:00076044</oboInOwl:id>
        <rdfs:label>Lekwa Local Municipality</rdfs:label>
    </owl:NamedIndividual>
    


    <!-- http://purl.obolibrary.org/obo/GAZ_00076045 -->

    <owl:NamedIndividual rdf:about="http://purl.obolibrary.org/obo/GAZ_00076045">
        <obo:RO_0001025 rdf:resource="http://purl.obolibrary.org/obo/GAZ_00032885"/>
        <obo:IAO_0000115>A local municipality in Gert Sibande District Municipality.</obo:IAO_0000115>
        <oboInOwl:hasOBONamespace>GAZ</oboInOwl:hasOBONamespace>
        <oboInOwl:id>GAZ:00076045</oboInOwl:id>
        <rdfs:label>Dipaleseng Local Municipality</rdfs:label>
    </owl:NamedIndividual>
    


    <!-- http://purl.obolibrary.org/obo/GAZ_00076046 -->

    <owl:NamedIndividual rdf:about="http://purl.obolibrary.org/obo/GAZ_00076046">
        <obo:RO_0001025 rdf:resource="http://purl.obolibrary.org/obo/GAZ_00032885"/>
        <obo:IAO_0000115>A local municipality in Gert Sibande District Municipality.</obo:IAO_0000115>
        <oboInOwl:hasOBONamespace>GAZ</oboInOwl:hasOBONamespace>
        <oboInOwl:id>GAZ:00076046</oboInOwl:id>
        <rdfs:label>Govan Mbeki Local Municipality</rdfs:label>
    </owl:NamedIndividual>
    


    <!-- http://purl.obolibrary.org/obo/GAZ_00076047 -->

    <owl:NamedIndividual rdf:about="http://purl.obolibrary.org/obo/GAZ_00076047">
        <obo:RO_0001025 rdf:resource="http://purl.obolibrary.org/obo/GAZ_00032885"/>
        <obo:IAO_0000115>A local municipality in Gert Sibande District Municipality.</obo:IAO_0000115>
        <oboInOwl:hasOBONamespace>GAZ</oboInOwl:hasOBONamespace>
        <oboInOwl:id>GAZ:00076047</oboInOwl:id>
        <rdfs:label>Mkhondo Local Municipality</rdfs:label>
    </owl:NamedIndividual>
    


    <!-- http://purl.obolibrary.org/obo/GAZ_00076048 -->

    <owl:NamedIndividual rdf:about="http://purl.obolibrary.org/obo/GAZ_00076048">
        <obo:RO_0001025 rdf:resource="http://purl.obolibrary.org/obo/GAZ_00032885"/>
        <obo:IAO_0000115>A local municipality in Gert Sibande District Municipality.</obo:IAO_0000115>
        <oboInOwl:hasOBONamespace>GAZ</oboInOwl:hasOBONamespace>
        <oboInOwl:id>GAZ:00076048</oboInOwl:id>
        <rdfs:label>Msukaligwa Local Municipality</rdfs:label>
    </owl:NamedIndividual>
    


    <!-- http://purl.obolibrary.org/obo/GAZ_00076049 -->

    <owl:NamedIndividual rdf:about="http://purl.obolibrary.org/obo/GAZ_00076049">
        <obo:RO_0001025 rdf:resource="http://purl.obolibrary.org/obo/GAZ_00032885"/>
        <obo:IAO_0000115>A local municipality in Gert Sibande District Municipality.</obo:IAO_0000115>
        <oboInOwl:hasOBONamespace>GAZ</oboInOwl:hasOBONamespace>
        <oboInOwl:id>GAZ:00076049</oboInOwl:id>
        <rdfs:label>Pixley Ka Seme Local Municipality</rdfs:label>
    </owl:NamedIndividual>
    


    <!-- http://purl.obolibrary.org/obo/GAZ_00076050 -->

    <owl:NamedIndividual rdf:about="http://purl.obolibrary.org/obo/GAZ_00076050">
        <obo:RO_0001025 rdf:resource="http://purl.obolibrary.org/obo/GAZ_00032885"/>
        <obo:IAO_0000115>A local municipality in Gert Sibande District Municipality.</obo:IAO_0000115>
        <oboInOwl:hasOBONamespace>GAZ</oboInOwl:hasOBONamespace>
        <oboInOwl:id>GAZ:00076050</oboInOwl:id>
        <rdfs:label>Albert Luthuli Local Municipality</rdfs:label>
    </owl:NamedIndividual>
    


    <!-- http://purl.obolibrary.org/obo/GAZ_00076051 -->

    <owl:NamedIndividual rdf:about="http://purl.obolibrary.org/obo/GAZ_00076051">
        <obo:RO_0001025 rdf:resource="http://purl.obolibrary.org/obo/GAZ_00032886"/>
        <obo:IAO_0000115>A local municipality in Nkangala District Municipality.</obo:IAO_0000115>
        <oboInOwl:hasOBONamespace>GAZ</oboInOwl:hasOBONamespace>
        <oboInOwl:id>GAZ:00076051</oboInOwl:id>
        <rdfs:label>Highlands Local Municipality</rdfs:label>
    </owl:NamedIndividual>
    


    <!-- http://purl.obolibrary.org/obo/GAZ_00076052 -->

    <owl:NamedIndividual rdf:about="http://purl.obolibrary.org/obo/GAZ_00076052">
        <obo:RO_0001025 rdf:resource="http://purl.obolibrary.org/obo/GAZ_00032886"/>
        <obo:IAO_0000115>A local municipality in Nkangala District Municipality.</obo:IAO_0000115>
        <oboInOwl:hasOBONamespace>GAZ</oboInOwl:hasOBONamespace>
        <oboInOwl:id>GAZ:00076052</oboInOwl:id>
        <rdfs:label>Emalahleni Local Municipality</rdfs:label>
    </owl:NamedIndividual>
    


    <!-- http://purl.obolibrary.org/obo/GAZ_00076053 -->

    <owl:NamedIndividual rdf:about="http://purl.obolibrary.org/obo/GAZ_00076053">
        <obo:RO_0001025 rdf:resource="http://purl.obolibrary.org/obo/GAZ_00032886"/>
        <obo:IAO_0000115>A local municipality in Nkangala District Municipality.</obo:IAO_0000115>
        <oboInOwl:hasOBONamespace>GAZ</oboInOwl:hasOBONamespace>
        <oboInOwl:id>GAZ:00076053</oboInOwl:id>
        <rdfs:label>Dr JS Moroka Local Municipality</rdfs:label>
    </owl:NamedIndividual>
    


    <!-- http://purl.obolibrary.org/obo/GAZ_00076054 -->

    <owl:NamedIndividual rdf:about="http://purl.obolibrary.org/obo/GAZ_00076054">
        <obo:RO_0001025 rdf:resource="http://purl.obolibrary.org/obo/GAZ_00032886"/>
        <obo:IAO_0000115>A local municipality in Nkangala District Municipality.</obo:IAO_0000115>
        <oboInOwl:hasOBONamespace>GAZ</oboInOwl:hasOBONamespace>
        <oboInOwl:id>GAZ:00076054</oboInOwl:id>
        <rdfs:label>Steve Tshwete Local Municipality</rdfs:label>
    </owl:NamedIndividual>
    


    <!-- http://purl.obolibrary.org/obo/GAZ_00076055 -->

    <owl:NamedIndividual rdf:about="http://purl.obolibrary.org/obo/GAZ_00076055">
        <obo:RO_0001025 rdf:resource="http://purl.obolibrary.org/obo/GAZ_00032886"/>
        <obo:IAO_0000115>A local municipality in Nkangala District Municipality.</obo:IAO_0000115>
        <oboInOwl:hasOBONamespace>GAZ</oboInOwl:hasOBONamespace>
        <oboInOwl:id>GAZ:00076055</oboInOwl:id>
        <rdfs:label>Delmas Local Municipality</rdfs:label>
    </owl:NamedIndividual>
    


    <!-- http://purl.obolibrary.org/obo/GAZ_00076056 -->

    <owl:NamedIndividual rdf:about="http://purl.obolibrary.org/obo/GAZ_00076056">
        <obo:RO_0001025 rdf:resource="http://purl.obolibrary.org/obo/GAZ_00032886"/>
        <obo:IAO_0000115>A local municipality in Nkangala District Municipality.</obo:IAO_0000115>
        <oboInOwl:hasOBONamespace>GAZ</oboInOwl:hasOBONamespace>
        <oboInOwl:id>GAZ:00076056</oboInOwl:id>
        <rdfs:label>Thembisile Local Municipality</rdfs:label>
    </owl:NamedIndividual>
    


    <!-- http://purl.obolibrary.org/obo/GAZ_00076057 -->

    <owl:NamedIndividual rdf:about="http://purl.obolibrary.org/obo/GAZ_00076057">
        <obo:RO_0001025 rdf:resource="http://purl.obolibrary.org/obo/GAZ_00032887"/>
        <obo:IAO_0000115>A local municipality of South Africa, located in the Ehlanzeni District Municipality, Mpumalanga. The municipality was formed in 2000 by the merger of Hazyview, Nelspruit, and White River local councils.</obo:IAO_0000115>
        <oboInOwl:hasOBONamespace>GAZ</oboInOwl:hasOBONamespace>
        <oboInOwl:id>GAZ:00076057</oboInOwl:id>
        <rdfs:label>Mbombela Local Municipality</rdfs:label>
    </owl:NamedIndividual>
    


    <!-- http://purl.obolibrary.org/obo/GAZ_00076058 -->

    <owl:NamedIndividual rdf:about="http://purl.obolibrary.org/obo/GAZ_00076058">
        <obo:RO_0001025 rdf:resource="http://purl.obolibrary.org/obo/GAZ_00032887"/>
        <obo:IAO_0000115>A local municipality in Ehlanzeni District Municipality.</obo:IAO_0000115>
        <oboInOwl:hasOBONamespace>GAZ</oboInOwl:hasOBONamespace>
        <oboInOwl:id>GAZ:00076058</oboInOwl:id>
        <rdfs:label>Nkomazi Local Municipality</rdfs:label>
    </owl:NamedIndividual>
    


    <!-- http://purl.obolibrary.org/obo/GAZ_00076059 -->

    <owl:NamedIndividual rdf:about="http://purl.obolibrary.org/obo/GAZ_00076059">
        <obo:RO_0001025 rdf:resource="http://purl.obolibrary.org/obo/GAZ_00032887"/>
        <obo:IAO_0000115>A local municipality in Ehlanzeni District Municipality.</obo:IAO_0000115>
        <oboInOwl:hasOBONamespace>GAZ</oboInOwl:hasOBONamespace>
        <oboInOwl:id>GAZ:00076059</oboInOwl:id>
        <rdfs:label>Thaba Chweu Local Municipality</rdfs:label>
    </owl:NamedIndividual>
    


    <!-- http://purl.obolibrary.org/obo/GAZ_00076060 -->

    <owl:NamedIndividual rdf:about="http://purl.obolibrary.org/obo/GAZ_00076060">
        <obo:RO_0001025 rdf:resource="http://purl.obolibrary.org/obo/GAZ_00032887"/>
        <obo:IAO_0000115>A local municipality in Ehlanzeni District Municipality.</obo:IAO_0000115>
        <oboInOwl:hasOBONamespace>GAZ</oboInOwl:hasOBONamespace>
        <oboInOwl:id>GAZ:00076060</oboInOwl:id>
        <rdfs:label>Umjindi Local Municipality</rdfs:label>
    </owl:NamedIndividual>
    


    <!-- http://purl.obolibrary.org/obo/GAZ_00076061 -->

    <owl:NamedIndividual rdf:about="http://purl.obolibrary.org/obo/GAZ_00076061">
        <obo:RO_0001025 rdf:resource="http://purl.obolibrary.org/obo/GAZ_00032887"/>
        <obo:IAO_0000115>A local municipality in Ehlanzeni District Municipality.</obo:IAO_0000115>
        <oboInOwl:hasOBONamespace>GAZ</oboInOwl:hasOBONamespace>
        <oboInOwl:id>GAZ:00076061</oboInOwl:id>
        <rdfs:label>Bushbuckridge Local Municipality</rdfs:label>
    </owl:NamedIndividual>
    


    <!-- http://purl.obolibrary.org/obo/GAZ_00076062 -->

    <owl:NamedIndividual rdf:about="http://purl.obolibrary.org/obo/GAZ_00076062">
        <obo:RO_0001025 rdf:resource="http://purl.obolibrary.org/obo/GAZ_00032877"/>
        <obo:IAO_0000115>A local municipality located in Bojanala Platinum District Municipality. In the North West province of South Africa.</obo:IAO_0000115>
        <oboInOwl:hasOBONamespace>GAZ</oboInOwl:hasOBONamespace>
        <oboInOwl:id>GAZ:00076062</oboInOwl:id>
        <rdfs:label>Rustenburg Local Municipality</rdfs:label>
    </owl:NamedIndividual>
    


    <!-- http://purl.obolibrary.org/obo/GAZ_00076063 -->

    <owl:NamedIndividual rdf:about="http://purl.obolibrary.org/obo/GAZ_00076063">
        <obo:RO_0001025 rdf:resource="http://purl.obolibrary.org/obo/GAZ_00032877"/>
        <obo:IAO_0000115>A local municipality located in Bojanala Platinum District Municipality. It is in the North West province of South Africa.</obo:IAO_0000115>
        <oboInOwl:hasOBONamespace>GAZ</oboInOwl:hasOBONamespace>
        <oboInOwl:id>GAZ:00076063</oboInOwl:id>
        <rdfs:label>Moretele Local Municipality</rdfs:label>
    </owl:NamedIndividual>
    


    <!-- http://purl.obolibrary.org/obo/GAZ_00076065 -->

    <owl:NamedIndividual rdf:about="http://purl.obolibrary.org/obo/GAZ_00076065">
        <obo:RO_0001025 rdf:resource="http://purl.obolibrary.org/obo/GAZ_00032877"/>
        <obo:IAO_0000115>A local municipality located in Bojanala Platinum District Municipality. It is in the North West province of South Africa.</obo:IAO_0000115>
        <oboInOwl:hasOBONamespace>GAZ</oboInOwl:hasOBONamespace>
        <oboInOwl:id>GAZ:00076065</oboInOwl:id>
        <rdfs:label>Madibeng Local Municipality</rdfs:label>
    </owl:NamedIndividual>
    


    <!-- http://purl.obolibrary.org/obo/GAZ_00076066 -->

    <owl:NamedIndividual rdf:about="http://purl.obolibrary.org/obo/GAZ_00076066">
        <obo:RO_0001025 rdf:resource="http://purl.obolibrary.org/obo/GAZ_00032877"/>
        <obo:IAO_0000115>A local municipality located in Bojanala Platinum District Municipality. It is in the North West province of South Africa.</obo:IAO_0000115>
        <oboInOwl:hasOBONamespace>GAZ</oboInOwl:hasOBONamespace>
        <oboInOwl:id>GAZ:00076066</oboInOwl:id>
        <rdfs:label>Moses Kotane Local Municipality</rdfs:label>
    </owl:NamedIndividual>
    


    <!-- http://purl.obolibrary.org/obo/GAZ_00076067 -->

    <owl:NamedIndividual rdf:about="http://purl.obolibrary.org/obo/GAZ_00076067">
        <obo:RO_0001025 rdf:resource="http://purl.obolibrary.org/obo/GAZ_00032877"/>
        <obo:IAO_0000115>A local municipality located in Bojanala Platinum District Municipality. It is in the North West province of South Africa.</obo:IAO_0000115>
        <oboInOwl:hasOBONamespace>GAZ</oboInOwl:hasOBONamespace>
        <oboInOwl:id>GAZ:00076067</oboInOwl:id>
        <rdfs:label>Kgetlengrivier Local Municipality</rdfs:label>
    </owl:NamedIndividual>
    


    <!-- http://purl.obolibrary.org/obo/GAZ_00076068 -->

    <owl:NamedIndividual rdf:about="http://purl.obolibrary.org/obo/GAZ_00076068">
        <obo:RO_0001025 rdf:resource="http://purl.obolibrary.org/obo/GAZ_00032874"/>
        <obo:IAO_0000115>A local Municipality consisting of the towns of Delareyville, Sannieshof and Ottosdal in the Central District Municipality situated in the North West Province of South Africa.</obo:IAO_0000115>
        <oboInOwl:hasOBONamespace>GAZ</oboInOwl:hasOBONamespace>
        <oboInOwl:id>GAZ:00076068</oboInOwl:id>
        <rdfs:label>Tswaing Local Municipality</rdfs:label>
    </owl:NamedIndividual>
    


    <!-- http://purl.obolibrary.org/obo/GAZ_00076069 -->

    <owl:NamedIndividual rdf:about="http://purl.obolibrary.org/obo/GAZ_00076069">
        <obo:RO_0001025 rdf:resource="http://purl.obolibrary.org/obo/GAZ_00032874"/>
        <obo:IAO_0000115>A local municipality in Central District Municipality.</obo:IAO_0000115>
        <oboInOwl:hasOBONamespace>GAZ</oboInOwl:hasOBONamespace>
        <oboInOwl:id>GAZ:00076069</oboInOwl:id>
        <rdfs:label>Ratlou Local Municipality</rdfs:label>
    </owl:NamedIndividual>
    


    <!-- http://purl.obolibrary.org/obo/GAZ_00076070 -->

    <owl:NamedIndividual rdf:about="http://purl.obolibrary.org/obo/GAZ_00076070">
        <obo:RO_0001025 rdf:resource="http://purl.obolibrary.org/obo/GAZ_00032874"/>
        <obo:IAO_0000115>A local municipality in Central District Municipality.</obo:IAO_0000115>
        <oboInOwl:hasOBONamespace>GAZ</oboInOwl:hasOBONamespace>
        <oboInOwl:id>GAZ:00076070</oboInOwl:id>
        <rdfs:label>Ramotshere Moiloa Local Municipality</rdfs:label>
    </owl:NamedIndividual>
    


    <!-- http://purl.obolibrary.org/obo/GAZ_00076071 -->

    <owl:NamedIndividual rdf:about="http://purl.obolibrary.org/obo/GAZ_00076071">
        <obo:RO_0001025 rdf:resource="http://purl.obolibrary.org/obo/GAZ_00032874"/>
        <obo:IAO_0000115>A local municipality in Central District Municipality.</obo:IAO_0000115>
        <oboInOwl:hasOBONamespace>GAZ</oboInOwl:hasOBONamespace>
        <oboInOwl:id>GAZ:00076071</oboInOwl:id>
        <rdfs:label>Ditsobotla Local Municipality</rdfs:label>
    </owl:NamedIndividual>
    


    <!-- http://purl.obolibrary.org/obo/GAZ_00076072 -->

    <owl:NamedIndividual rdf:about="http://purl.obolibrary.org/obo/GAZ_00076072">
        <obo:RO_0001025 rdf:resource="http://purl.obolibrary.org/obo/GAZ_00032874"/>
        <obo:IAO_0000115>A local municipality in Central District Municipality.</obo:IAO_0000115>
        <oboInOwl:hasOBONamespace>GAZ</oboInOwl:hasOBONamespace>
        <oboInOwl:id>GAZ:00076072</oboInOwl:id>
        <rdfs:label>Mafikeng Local Municipality</rdfs:label>
    </owl:NamedIndividual>
    


    <!-- http://purl.obolibrary.org/obo/GAZ_00076073 -->

    <owl:NamedIndividual rdf:about="http://purl.obolibrary.org/obo/GAZ_00076073">
        <obo:RO_0001025 rdf:resource="http://purl.obolibrary.org/obo/GAZ_00032876"/>
        <obo:IAO_0000115>A local municipality in Bophirima District Municipality.</obo:IAO_0000115>
        <oboInOwl:hasOBONamespace>GAZ</oboInOwl:hasOBONamespace>
        <oboInOwl:id>GAZ:00076073</oboInOwl:id>
        <rdfs:label>Naledi Local Municipality</rdfs:label>
    </owl:NamedIndividual>
    


    <!-- http://purl.obolibrary.org/obo/GAZ_00076074 -->

    <owl:NamedIndividual rdf:about="http://purl.obolibrary.org/obo/GAZ_00076074">
        <obo:RO_0001025 rdf:resource="http://purl.obolibrary.org/obo/GAZ_00032876"/>
        <obo:IAO_0000115>A local municipality in Bophirima District Municipality.</obo:IAO_0000115>
        <oboInOwl:hasOBONamespace>GAZ</oboInOwl:hasOBONamespace>
        <oboInOwl:id>GAZ:00076074</oboInOwl:id>
        <rdfs:label>Kagisano Local Municipality</rdfs:label>
    </owl:NamedIndividual>
    


    <!-- http://purl.obolibrary.org/obo/GAZ_00076075 -->

    <owl:NamedIndividual rdf:about="http://purl.obolibrary.org/obo/GAZ_00076075">
        <obo:RO_0001025 rdf:resource="http://purl.obolibrary.org/obo/GAZ_00032876"/>
        <obo:IAO_0000115>A local municipality in Bophirima District Municipality.</obo:IAO_0000115>
        <oboInOwl:hasOBONamespace>GAZ</oboInOwl:hasOBONamespace>
        <oboInOwl:id>GAZ:00076075</oboInOwl:id>
        <rdfs:label>Lekwa-Teemane Local Municipality</rdfs:label>
    </owl:NamedIndividual>
    


    <!-- http://purl.obolibrary.org/obo/GAZ_00076076 -->

    <owl:NamedIndividual rdf:about="http://purl.obolibrary.org/obo/GAZ_00076076">
        <obo:RO_0001025 rdf:resource="http://purl.obolibrary.org/obo/GAZ_00032876"/>
        <obo:IAO_0000115>A local municipality in Bophirima District Municipality.</obo:IAO_0000115>
        <oboInOwl:hasOBONamespace>GAZ</oboInOwl:hasOBONamespace>
        <oboInOwl:id>GAZ:00076076</oboInOwl:id>
        <rdfs:label>Mamusa Local Municipality</rdfs:label>
    </owl:NamedIndividual>
    


    <!-- http://purl.obolibrary.org/obo/GAZ_00076077 -->

    <owl:NamedIndividual rdf:about="http://purl.obolibrary.org/obo/GAZ_00076077">
        <obo:RO_0001025 rdf:resource="http://purl.obolibrary.org/obo/GAZ_00032876"/>
        <obo:IAO_0000115>A local municipality in Bophirima District Municipality.</obo:IAO_0000115>
        <oboInOwl:hasOBONamespace>GAZ</oboInOwl:hasOBONamespace>
        <oboInOwl:id>GAZ:00076077</oboInOwl:id>
        <rdfs:label>Greater Taung Local Municipality</rdfs:label>
    </owl:NamedIndividual>
    


    <!-- http://purl.obolibrary.org/obo/GAZ_00076078 -->

    <owl:NamedIndividual rdf:about="http://purl.obolibrary.org/obo/GAZ_00076078">
        <obo:RO_0001025 rdf:resource="http://purl.obolibrary.org/obo/GAZ_00032876"/>
        <obo:IAO_0000115>A local municipality in Bophirima District Municipality.</obo:IAO_0000115>
        <oboInOwl:hasOBONamespace>GAZ</oboInOwl:hasOBONamespace>
        <oboInOwl:id>GAZ:00076078</oboInOwl:id>
        <rdfs:label>Molopo Local Municipality</rdfs:label>
    </owl:NamedIndividual>
    


    <!-- http://purl.obolibrary.org/obo/GAZ_00076079 -->

    <owl:NamedIndividual rdf:about="http://purl.obolibrary.org/obo/GAZ_00076079">
        <obo:RO_0001025 rdf:resource="http://purl.obolibrary.org/obo/GAZ_00032875"/>
        <obo:IAO_0000115>A local municipality in Southern District Municipality, North West, South Africa.</obo:IAO_0000115>
        <oboInOwl:hasOBONamespace>GAZ</oboInOwl:hasOBONamespace>
        <oboInOwl:id>GAZ:00076079</oboInOwl:id>
        <rdfs:label>Maquassi Hills Local Municipality</rdfs:label>
    </owl:NamedIndividual>
    


    <!-- http://purl.obolibrary.org/obo/GAZ_00076080 -->

    <owl:NamedIndividual rdf:about="http://purl.obolibrary.org/obo/GAZ_00076080">
        <obo:RO_0001025 rdf:resource="http://purl.obolibrary.org/obo/GAZ_00032875"/>
        <obo:IAO_0000115>A local municipality in Southern District Municipality, North West, South Africa.</obo:IAO_0000115>
        <oboInOwl:hasOBONamespace>GAZ</oboInOwl:hasOBONamespace>
        <oboInOwl:id>GAZ:00076080</oboInOwl:id>
        <rdfs:label>Matlosana Local Municipality</rdfs:label>
    </owl:NamedIndividual>
    


    <!-- http://purl.obolibrary.org/obo/GAZ_00076081 -->

    <owl:NamedIndividual rdf:about="http://purl.obolibrary.org/obo/GAZ_00076081">
        <obo:RO_0001025 rdf:resource="http://purl.obolibrary.org/obo/GAZ_00032875"/>
        <obo:IAO_0000115>A local municipality in Southern District Municipality, North West, South Africa.</obo:IAO_0000115>
        <oboInOwl:hasOBONamespace>GAZ</oboInOwl:hasOBONamespace>
        <oboInOwl:id>GAZ:00076081</oboInOwl:id>
        <rdfs:label>Merafong City Local Municipality</rdfs:label>
    </owl:NamedIndividual>
    


    <!-- http://purl.obolibrary.org/obo/GAZ_00076082 -->

    <owl:NamedIndividual rdf:about="http://purl.obolibrary.org/obo/GAZ_00076082">
        <obo:RO_0001025 rdf:resource="http://purl.obolibrary.org/obo/GAZ_00032875"/>
        <obo:IAO_0000115>A local municipality in Southern District Municipality, North West, South Africa.</obo:IAO_0000115>
        <oboInOwl:hasOBONamespace>GAZ</oboInOwl:hasOBONamespace>
        <oboInOwl:id>GAZ:00076082</oboInOwl:id>
        <rdfs:label>Ventersdorp Local Municipality</rdfs:label>
    </owl:NamedIndividual>
    


    <!-- http://purl.obolibrary.org/obo/GAZ_00076083 -->

    <owl:NamedIndividual rdf:about="http://purl.obolibrary.org/obo/GAZ_00076083">
        <obo:RO_0001025 rdf:resource="http://purl.obolibrary.org/obo/GAZ_00032872"/>
        <obo:IAO_0000115>A local municipality in Namakwa District Municipality.</obo:IAO_0000115>
        <oboInOwl:hasOBONamespace>GAZ</oboInOwl:hasOBONamespace>
        <oboInOwl:id>GAZ:00076083</oboInOwl:id>
        <rdfs:label>Nama Khoi Local Municipality</rdfs:label>
    </owl:NamedIndividual>
    


    <!-- http://purl.obolibrary.org/obo/GAZ_00076084 -->

    <owl:NamedIndividual rdf:about="http://purl.obolibrary.org/obo/GAZ_00076084">
        <obo:RO_0001025 rdf:resource="http://purl.obolibrary.org/obo/GAZ_00032872"/>
        <obo:IAO_0000115>A local municipality in Namakwa District Municipality.</obo:IAO_0000115>
        <oboInOwl:hasOBONamespace>GAZ</oboInOwl:hasOBONamespace>
        <oboInOwl:id>GAZ:00076084</oboInOwl:id>
        <rdfs:label>Khoi-Ma Local Municipality</rdfs:label>
    </owl:NamedIndividual>
    


    <!-- http://purl.obolibrary.org/obo/GAZ_00076085 -->

    <owl:NamedIndividual rdf:about="http://purl.obolibrary.org/obo/GAZ_00076085">
        <obo:RO_0001025 rdf:resource="http://purl.obolibrary.org/obo/GAZ_00032872"/>
        <obo:IAO_0000115>A local municipality in Namakwa District Municipality.</obo:IAO_0000115>
        <oboInOwl:hasOBONamespace>GAZ</oboInOwl:hasOBONamespace>
        <oboInOwl:id>GAZ:00076085</oboInOwl:id>
        <rdfs:label>Hantam Local Municipality</rdfs:label>
    </owl:NamedIndividual>
    


    <!-- http://purl.obolibrary.org/obo/GAZ_00076086 -->

    <owl:NamedIndividual rdf:about="http://purl.obolibrary.org/obo/GAZ_00076086">
        <obo:RO_0001025 rdf:resource="http://purl.obolibrary.org/obo/GAZ_00032872"/>
        <obo:IAO_0000115>A local municipality in Namakwa District Municipality.</obo:IAO_0000115>
        <oboInOwl:hasOBONamespace>GAZ</oboInOwl:hasOBONamespace>
        <oboInOwl:id>GAZ:00076086</oboInOwl:id>
        <rdfs:label>Richtersveld Local Municipality</rdfs:label>
    </owl:NamedIndividual>
    


    <!-- http://purl.obolibrary.org/obo/GAZ_00076087 -->

    <owl:NamedIndividual rdf:about="http://purl.obolibrary.org/obo/GAZ_00076087">
        <obo:RO_0001025 rdf:resource="http://purl.obolibrary.org/obo/GAZ_00032872"/>
        <obo:IAO_0000115>A local municipality in Namakwa District Municipality.</obo:IAO_0000115>
        <oboInOwl:hasOBONamespace>GAZ</oboInOwl:hasOBONamespace>
        <oboInOwl:id>GAZ:00076087</oboInOwl:id>
        <rdfs:label>Kamiesberg Local Municipality</rdfs:label>
    </owl:NamedIndividual>
    


    <!-- http://purl.obolibrary.org/obo/GAZ_00076088 -->

    <owl:NamedIndividual rdf:about="http://purl.obolibrary.org/obo/GAZ_00076088">
        <obo:RO_0001025 rdf:resource="http://purl.obolibrary.org/obo/GAZ_00032872"/>
        <obo:IAO_0000115>A local municipality in Namakwa District Municipality.</obo:IAO_0000115>
        <oboInOwl:hasOBONamespace>GAZ</oboInOwl:hasOBONamespace>
        <oboInOwl:id>GAZ:00076088</oboInOwl:id>
        <rdfs:label>Karoo Hoogland Local Municipality</rdfs:label>
    </owl:NamedIndividual>
    


    <!-- http://purl.obolibrary.org/obo/GAZ_00076089 -->

    <owl:NamedIndividual rdf:about="http://purl.obolibrary.org/obo/GAZ_00076089">
        <obo:RO_0001025 rdf:resource="http://purl.obolibrary.org/obo/GAZ_00032871"/>
        <obo:IAO_0000115>A local municipality in Karoo District Municipality.</obo:IAO_0000115>
        <oboInOwl:hasOBONamespace>GAZ</oboInOwl:hasOBONamespace>
        <oboInOwl:id>GAZ:00076089</oboInOwl:id>
        <rdfs:label>Umsobomvu Local Municipality</rdfs:label>
    </owl:NamedIndividual>
    


    <!-- http://purl.obolibrary.org/obo/GAZ_00076090 -->

    <owl:NamedIndividual rdf:about="http://purl.obolibrary.org/obo/GAZ_00076090">
        <obo:RO_0001025 rdf:resource="http://purl.obolibrary.org/obo/GAZ_00032871"/>
        <obo:IAO_0000115>A local municipality in Karoo District Municipality.</obo:IAO_0000115>
        <oboInOwl:hasOBONamespace>GAZ</oboInOwl:hasOBONamespace>
        <oboInOwl:id>GAZ:00076090</oboInOwl:id>
        <rdfs:label>Renosterberg Local Municipality</rdfs:label>
    </owl:NamedIndividual>
    


    <!-- http://purl.obolibrary.org/obo/GAZ_00076091 -->

    <owl:NamedIndividual rdf:about="http://purl.obolibrary.org/obo/GAZ_00076091">
        <obo:RO_0001025 rdf:resource="http://purl.obolibrary.org/obo/GAZ_00032871"/>
        <obo:IAO_0000115>A local municipality in Karoo District Municipality.</obo:IAO_0000115>
        <oboInOwl:hasOBONamespace>GAZ</oboInOwl:hasOBONamespace>
        <oboInOwl:id>GAZ:00076091</oboInOwl:id>
        <rdfs:label>Emthanjeni Local Municipality</rdfs:label>
    </owl:NamedIndividual>
    


    <!-- http://purl.obolibrary.org/obo/GAZ_00076092 -->

    <owl:NamedIndividual rdf:about="http://purl.obolibrary.org/obo/GAZ_00076092">
        <obo:RO_0001025 rdf:resource="http://purl.obolibrary.org/obo/GAZ_00032871"/>
        <obo:IAO_0000115>A local municipality in Karoo District Municipality.</obo:IAO_0000115>
        <oboInOwl:hasOBONamespace>GAZ</oboInOwl:hasOBONamespace>
        <oboInOwl:id>GAZ:00076092</oboInOwl:id>
        <rdfs:label>Thembelihle Local Municipality</rdfs:label>
    </owl:NamedIndividual>
    


    <!-- http://purl.obolibrary.org/obo/GAZ_00076093 -->

    <owl:NamedIndividual rdf:about="http://purl.obolibrary.org/obo/GAZ_00076093">
        <obo:RO_0001025 rdf:resource="http://purl.obolibrary.org/obo/GAZ_00032871"/>
        <obo:IAO_0000115>A local municipality in Karoo District Municipality.</obo:IAO_0000115>
        <oboInOwl:hasOBONamespace>GAZ</oboInOwl:hasOBONamespace>
        <oboInOwl:id>GAZ:00076093</oboInOwl:id>
        <rdfs:label>Kareeberg Local Municipality</rdfs:label>
    </owl:NamedIndividual>
    


    <!-- http://purl.obolibrary.org/obo/GAZ_00076094 -->

    <owl:NamedIndividual rdf:about="http://purl.obolibrary.org/obo/GAZ_00076094">
        <obo:RO_0001025 rdf:resource="http://purl.obolibrary.org/obo/GAZ_00032871"/>
        <obo:IAO_0000115>A lDistrict Management Area in Karoo District Municipality.</obo:IAO_0000115>
        <oboInOwl:hasOBONamespace>GAZ</oboInOwl:hasOBONamespace>
        <oboInOwl:id>GAZ:00076094</oboInOwl:id>
        <rdfs:label>Bo Karoo District Management Area</rdfs:label>
    </owl:NamedIndividual>
    


    <!-- http://purl.obolibrary.org/obo/GAZ_00076095 -->

    <owl:NamedIndividual rdf:about="http://purl.obolibrary.org/obo/GAZ_00076095">
        <obo:RO_0001025 rdf:resource="http://purl.obolibrary.org/obo/GAZ_00032871"/>
        <obo:IAO_0000115>A local municipality in Karoo District Municipality.</obo:IAO_0000115>
        <oboInOwl:hasOBONamespace>GAZ</oboInOwl:hasOBONamespace>
        <oboInOwl:id>GAZ:00076095</oboInOwl:id>
        <rdfs:label>Siyancuma Local Municipality</rdfs:label>
    </owl:NamedIndividual>
    


    <!-- http://purl.obolibrary.org/obo/GAZ_00076096 -->

    <owl:NamedIndividual rdf:about="http://purl.obolibrary.org/obo/GAZ_00076096">
        <obo:RO_0001025 rdf:resource="http://purl.obolibrary.org/obo/GAZ_00032871"/>
        <obo:IAO_0000115>A local municipality in Karoo District Municipality.</obo:IAO_0000115>
        <oboInOwl:hasOBONamespace>GAZ</oboInOwl:hasOBONamespace>
        <oboInOwl:id>GAZ:00076096</oboInOwl:id>
        <rdfs:label>Ubuntu Local Municipality</rdfs:label>
    </owl:NamedIndividual>
    


    <!-- http://purl.obolibrary.org/obo/GAZ_00076097 -->

    <owl:NamedIndividual rdf:about="http://purl.obolibrary.org/obo/GAZ_00076097">
        <obo:RO_0001025 rdf:resource="http://purl.obolibrary.org/obo/GAZ_00032871"/>
        <obo:IAO_0000115>A local municipality in Karoo District Municipality.</obo:IAO_0000115>
        <oboInOwl:hasOBONamespace>GAZ</oboInOwl:hasOBONamespace>
        <oboInOwl:id>GAZ:00076097</oboInOwl:id>
        <rdfs:label>Siyathemba Local Municipality</rdfs:label>
    </owl:NamedIndividual>
    


    <!-- http://purl.obolibrary.org/obo/GAZ_00076098 -->

    <owl:NamedIndividual rdf:about="http://purl.obolibrary.org/obo/GAZ_00076098">
        <obo:RO_0001025 rdf:resource="http://purl.obolibrary.org/obo/GAZ_00032873"/>
        <obo:IAO_0000115>A local municipality in Siyanda District Municipality.</obo:IAO_0000115>
        <oboInOwl:hasOBONamespace>GAZ</oboInOwl:hasOBONamespace>
        <oboInOwl:id>GAZ:00076098</oboInOwl:id>
        <rdfs:label>Kheis Local Municipality</rdfs:label>
    </owl:NamedIndividual>
    


    <!-- http://purl.obolibrary.org/obo/GAZ_00076100 -->

    <owl:NamedIndividual rdf:about="http://purl.obolibrary.org/obo/GAZ_00076100">
        <obo:RO_0001025 rdf:resource="http://purl.obolibrary.org/obo/GAZ_00032873"/>
        <obo:IAO_0000115>A local municipality in Siyanda District Municipality.</obo:IAO_0000115>
        <oboInOwl:hasOBONamespace>GAZ</oboInOwl:hasOBONamespace>
        <oboInOwl:id>GAZ:00076100</oboInOwl:id>
        <rdfs:label>Kai Garib Local Municipality</rdfs:label>
    </owl:NamedIndividual>
    


    <!-- http://purl.obolibrary.org/obo/GAZ_00076101 -->

    <owl:NamedIndividual rdf:about="http://purl.obolibrary.org/obo/GAZ_00076101">
        <obo:RO_0001025 rdf:resource="http://purl.obolibrary.org/obo/GAZ_00032873"/>
        <obo:IAO_0000115>A local municipality in Siyanda District Municipality.</obo:IAO_0000115>
        <oboInOwl:hasOBONamespace>GAZ</oboInOwl:hasOBONamespace>
        <oboInOwl:id>GAZ:00076101</oboInOwl:id>
        <rdfs:label>Tsantsabane Local Municipality</rdfs:label>
    </owl:NamedIndividual>
    


    <!-- http://purl.obolibrary.org/obo/GAZ_00076102 -->

    <owl:NamedIndividual rdf:about="http://purl.obolibrary.org/obo/GAZ_00076102">
        <obo:RO_0001025 rdf:resource="http://purl.obolibrary.org/obo/GAZ_00032873"/>
        <obo:IAO_0000115>A local municipality in Siyanda District Municipality.</obo:IAO_0000115>
        <oboInOwl:hasOBONamespace>GAZ</oboInOwl:hasOBONamespace>
        <oboInOwl:id>GAZ:00076102</oboInOwl:id>
        <rdfs:label>Mier Local Municipality</rdfs:label>
    </owl:NamedIndividual>
    


    <!-- http://purl.obolibrary.org/obo/GAZ_00076103 -->

    <owl:NamedIndividual rdf:about="http://purl.obolibrary.org/obo/GAZ_00076103">
        <obo:RO_0001025 rdf:resource="http://purl.obolibrary.org/obo/GAZ_00032873"/>
        <obo:IAO_0000115>A local municipality in Siyanda District Municipality.</obo:IAO_0000115>
        <oboInOwl:hasOBONamespace>GAZ</oboInOwl:hasOBONamespace>
        <oboInOwl:id>GAZ:00076103</oboInOwl:id>
        <rdfs:label>Khara Hais Local Municipality</rdfs:label>
    </owl:NamedIndividual>
    


    <!-- http://purl.obolibrary.org/obo/GAZ_00076104 -->

    <owl:NamedIndividual rdf:about="http://purl.obolibrary.org/obo/GAZ_00076104">
        <obo:RO_0001025 rdf:resource="http://purl.obolibrary.org/obo/GAZ_00032870"/>
        <obo:IAO_0000115>A District Management Area in Frances Baard District Municipality.</obo:IAO_0000115>
        <oboInOwl:hasOBONamespace>GAZ</oboInOwl:hasOBONamespace>
        <oboInOwl:id>GAZ:00076104</oboInOwl:id>
        <rdfs:label>Diamondfields District Management Area</rdfs:label>
    </owl:NamedIndividual>
    


    <!-- http://purl.obolibrary.org/obo/GAZ_00076105 -->

    <owl:NamedIndividual rdf:about="http://purl.obolibrary.org/obo/GAZ_00076105">
        <obo:RO_0001025 rdf:resource="http://purl.obolibrary.org/obo/GAZ_00032870"/>
        <obo:IAO_0000115>A local municipality in Frances Baard District Municipality.</obo:IAO_0000115>
        <oboInOwl:hasOBONamespace>GAZ</oboInOwl:hasOBONamespace>
        <oboInOwl:id>GAZ:00076105</oboInOwl:id>
        <rdfs:label>Dikgatlong Local Municipality</rdfs:label>
    </owl:NamedIndividual>
    


    <!-- http://purl.obolibrary.org/obo/GAZ_00076106 -->

    <owl:NamedIndividual rdf:about="http://purl.obolibrary.org/obo/GAZ_00076106">
        <obo:RO_0001025 rdf:resource="http://purl.obolibrary.org/obo/GAZ_00032870"/>
        <obo:IAO_0000115>A local municipality in Frances Baard District Municipality.</obo:IAO_0000115>
        <oboInOwl:hasOBONamespace>GAZ</oboInOwl:hasOBONamespace>
        <oboInOwl:id>GAZ:00076106</oboInOwl:id>
        <rdfs:label>Phokwane Local Municipality</rdfs:label>
    </owl:NamedIndividual>
    


    <!-- http://purl.obolibrary.org/obo/GAZ_00076107 -->

    <owl:NamedIndividual rdf:about="http://purl.obolibrary.org/obo/GAZ_00076107">
        <obo:RO_0001025 rdf:resource="http://purl.obolibrary.org/obo/GAZ_00032870"/>
        <obo:IAO_0000115>A local municipality in Frances Baard District Municipality.</obo:IAO_0000115>
        <oboInOwl:hasOBONamespace>GAZ</oboInOwl:hasOBONamespace>
        <oboInOwl:id>GAZ:00076107</oboInOwl:id>
        <rdfs:label>Magareng Local Municipality</rdfs:label>
    </owl:NamedIndividual>
    


    <!-- http://purl.obolibrary.org/obo/GAZ_00076108 -->

    <owl:NamedIndividual rdf:about="http://purl.obolibrary.org/obo/GAZ_00076108">
        <obo:RO_0001025 rdf:resource="http://purl.obolibrary.org/obo/GAZ_00032870"/>
        <obo:IAO_0000115>A local municipality in Frances Baard District Municipality.</obo:IAO_0000115>
        <oboInOwl:hasOBONamespace>GAZ</oboInOwl:hasOBONamespace>
        <oboInOwl:id>GAZ:00076108</oboInOwl:id>
        <rdfs:label>Sol Plaatjie Local Municipality</rdfs:label>
    </owl:NamedIndividual>
    


    <!-- http://purl.obolibrary.org/obo/GAZ_00076109 -->

    <owl:NamedIndividual rdf:about="http://purl.obolibrary.org/obo/GAZ_00076109">
        <obo:RO_0001025 rdf:resource="http://purl.obolibrary.org/obo/GAZ_00032869"/>
        <obo:IAO_0000115>A local municipality in Kgalagadi District Municipality.</obo:IAO_0000115>
        <oboInOwl:hasOBONamespace>GAZ</oboInOwl:hasOBONamespace>
        <oboInOwl:id>GAZ:00076109</oboInOwl:id>
        <rdfs:label>Kalahari Local Municipality</rdfs:label>
    </owl:NamedIndividual>
    


    <!-- http://purl.obolibrary.org/obo/GAZ_00076110 -->

    <owl:NamedIndividual rdf:about="http://purl.obolibrary.org/obo/GAZ_00076110">
        <obo:RO_0001025 rdf:resource="http://purl.obolibrary.org/obo/GAZ_00032869"/>
        <obo:IAO_0000115>A local municipality in Kgalagadi District Municipality.</obo:IAO_0000115>
        <oboInOwl:hasOBONamespace>GAZ</oboInOwl:hasOBONamespace>
        <oboInOwl:id>GAZ:00076110</oboInOwl:id>
        <rdfs:label>Ga-Segonyana Local Municipality</rdfs:label>
    </owl:NamedIndividual>
    


    <!-- http://purl.obolibrary.org/obo/GAZ_00076111 -->

    <owl:NamedIndividual rdf:about="http://purl.obolibrary.org/obo/GAZ_00076111">
        <obo:RO_0001025 rdf:resource="http://purl.obolibrary.org/obo/GAZ_00032869"/>
        <obo:IAO_0000115>A local municipality in Kgalagadi District Municipality.</obo:IAO_0000115>
        <oboInOwl:hasOBONamespace>GAZ</oboInOwl:hasOBONamespace>
        <oboInOwl:id>GAZ:00076111</oboInOwl:id>
        <rdfs:label>Gamagara Local Municipality</rdfs:label>
    </owl:NamedIndividual>
    


    <!-- http://purl.obolibrary.org/obo/GAZ_00076112 -->

    <owl:NamedIndividual rdf:about="http://purl.obolibrary.org/obo/GAZ_00076112">
        <obo:RO_0001025 rdf:resource="http://purl.obolibrary.org/obo/GAZ_00032869"/>
        <obo:IAO_0000115>A local municipality in Kgalagadi District Municipality.</obo:IAO_0000115>
        <oboInOwl:hasOBONamespace>GAZ</oboInOwl:hasOBONamespace>
        <oboInOwl:id>GAZ:00076112</oboInOwl:id>
        <rdfs:label>Moshaweng Local Municipality</rdfs:label>
    </owl:NamedIndividual>
    


    <!-- http://purl.obolibrary.org/obo/GAZ_00076113 -->

    <owl:NamedIndividual rdf:about="http://purl.obolibrary.org/obo/GAZ_00076113">
        <obo:RO_0001025 rdf:resource="http://purl.obolibrary.org/obo/GAZ_00032856"/>
        <obo:IAO_0000115>A local municipality located in the Western Cape Province of South Africa.</obo:IAO_0000115>
        <oboInOwl:hasOBONamespace>GAZ</oboInOwl:hasOBONamespace>
        <oboInOwl:id>GAZ:00076113</oboInOwl:id>
        <rdfs:label>Bergrivier Local Municipality</rdfs:label>
    </owl:NamedIndividual>
    


    <!-- http://purl.obolibrary.org/obo/GAZ_00076114 -->

    <owl:NamedIndividual rdf:about="http://purl.obolibrary.org/obo/GAZ_00076114">
        <obo:RO_0001025 rdf:resource="http://purl.obolibrary.org/obo/GAZ_00032856"/>
        <obo:IAO_0000115>A local municipality located within the West Coast District Municipality, in the Western Cape Province of South Africa.</obo:IAO_0000115>
        <oboInOwl:hasOBONamespace>GAZ</oboInOwl:hasOBONamespace>
        <oboInOwl:id>GAZ:00076114</oboInOwl:id>
        <rdfs:label>Matzikama Local Municipality</rdfs:label>
    </owl:NamedIndividual>
    


    <!-- http://purl.obolibrary.org/obo/GAZ_00076115 -->

    <owl:NamedIndividual rdf:about="http://purl.obolibrary.org/obo/GAZ_00076115">
        <obo:RO_0001025 rdf:resource="http://purl.obolibrary.org/obo/GAZ_00012790"/>
        <obo:IAO_0000115>A local municipality located in the Western Cape Province of South Africa.</obo:IAO_0000115>
        <oboInOwl:hasOBONamespace>GAZ</oboInOwl:hasOBONamespace>
        <oboInOwl:id>GAZ:00076115</oboInOwl:id>
        <rdfs:label>Witzenberg Local Municipality</rdfs:label>
    </owl:NamedIndividual>
    


    <!-- http://purl.obolibrary.org/obo/GAZ_00076116 -->

    <owl:NamedIndividual rdf:about="http://purl.obolibrary.org/obo/GAZ_00076116">
        <obo:RO_0001025 rdf:resource="http://purl.obolibrary.org/obo/GAZ_00032856"/>
        <obo:IAO_0000115>A local municipality located in the Western Cape Province of South Africa.</obo:IAO_0000115>
        <oboInOwl:hasOBONamespace>GAZ</oboInOwl:hasOBONamespace>
        <oboInOwl:id>GAZ:00076116</oboInOwl:id>
        <rdfs:label>Cederberg Local Municipality</rdfs:label>
    </owl:NamedIndividual>
    


    <!-- http://purl.obolibrary.org/obo/GAZ_00076117 -->

    <owl:NamedIndividual rdf:about="http://purl.obolibrary.org/obo/GAZ_00076117">
        <obo:RO_0001025 rdf:resource="http://purl.obolibrary.org/obo/GAZ_00032856"/>
        <obo:IAO_0000115>A local municipality located in the Western Cape Province of South Africa.</obo:IAO_0000115>
        <oboInOwl:hasOBONamespace>GAZ</oboInOwl:hasOBONamespace>
        <oboInOwl:id>GAZ:00076117</oboInOwl:id>
        <rdfs:label>Swartland Local Municipality</rdfs:label>
    </owl:NamedIndividual>
    


    <!-- http://purl.obolibrary.org/obo/GAZ_00076118 -->

    <owl:NamedIndividual rdf:about="http://purl.obolibrary.org/obo/GAZ_00076118">
        <obo:RO_0001025 rdf:resource="http://purl.obolibrary.org/obo/GAZ_00032856"/>
        <obo:IAO_0000115>A local municipality located in the Western Cape Province of South Africa.</obo:IAO_0000115>
        <oboInOwl:hasOBONamespace>GAZ</oboInOwl:hasOBONamespace>
        <oboInOwl:id>GAZ:00076118</oboInOwl:id>
        <rdfs:label>Saldanha Bay Local Municipality</rdfs:label>
    </owl:NamedIndividual>
    


    <!-- http://purl.obolibrary.org/obo/GAZ_00076119 -->

    <owl:NamedIndividual rdf:about="http://purl.obolibrary.org/obo/GAZ_00076119">
        <obo:RO_0001025 rdf:resource="http://purl.obolibrary.org/obo/GAZ_00012790"/>
        <obo:IAO_0000115>A local municipality located in the Western Cape Province of South Africa.</obo:IAO_0000115>
        <oboInOwl:hasOBONamespace>GAZ</oboInOwl:hasOBONamespace>
        <oboInOwl:id>GAZ:00076119</oboInOwl:id>
        <rdfs:label>Breede River/Winelands Local Municipality</rdfs:label>
    </owl:NamedIndividual>
    


    <!-- http://purl.obolibrary.org/obo/GAZ_00076120 -->

    <owl:NamedIndividual rdf:about="http://purl.obolibrary.org/obo/GAZ_00076120">
        <obo:RO_0001025 rdf:resource="http://purl.obolibrary.org/obo/GAZ_00012792"/>
        <obo:IAO_0000115>A local municipality located in the Western Cape Province of South Africa.</obo:IAO_0000115>
        <oboInOwl:hasOBONamespace>GAZ</oboInOwl:hasOBONamespace>
        <oboInOwl:id>GAZ:00076120</oboInOwl:id>
        <rdfs:label>Oudtshoorn Local Municipality</rdfs:label>
    </owl:NamedIndividual>
    


    <!-- http://purl.obolibrary.org/obo/GAZ_00076121 -->

    <owl:NamedIndividual rdf:about="http://purl.obolibrary.org/obo/GAZ_00076121">
        <obo:RO_0001025 rdf:resource="http://purl.obolibrary.org/obo/GAZ_00012790"/>
        <obo:IAO_0000115>A local municipality located in the Western Cape Province of South Africa.</obo:IAO_0000115>
        <oboInOwl:hasOBONamespace>GAZ</oboInOwl:hasOBONamespace>
        <oboInOwl:id>GAZ:00076121</oboInOwl:id>
        <rdfs:label>Drakenstein Local Municipality</rdfs:label>
    </owl:NamedIndividual>
    


    <!-- http://purl.obolibrary.org/obo/GAZ_00076122 -->

    <owl:NamedIndividual rdf:about="http://purl.obolibrary.org/obo/GAZ_00076122">
        <obo:RO_0001025 rdf:resource="http://purl.obolibrary.org/obo/GAZ_00012790"/>
        <obo:IAO_0000115>A local municipality located in the Western Cape Province of South Africa.</obo:IAO_0000115>
        <oboInOwl:hasOBONamespace>GAZ</oboInOwl:hasOBONamespace>
        <oboInOwl:id>GAZ:00076122</oboInOwl:id>
        <rdfs:label>Breede Valley Local Municipality</rdfs:label>
    </owl:NamedIndividual>
    


    <!-- http://purl.obolibrary.org/obo/GAZ_00076123 -->

    <owl:NamedIndividual rdf:about="http://purl.obolibrary.org/obo/GAZ_00076123">
        <obo:RO_0001025 rdf:resource="http://purl.obolibrary.org/obo/GAZ_00032845"/>
        <obo:IAO_0000115>A local municipality located in the Western Cape Province of South Africa.</obo:IAO_0000115>
        <oboInOwl:hasOBONamespace>GAZ</oboInOwl:hasOBONamespace>
        <oboInOwl:id>GAZ:00076123</oboInOwl:id>
        <rdfs:label>Overstrand Local Municipality</rdfs:label>
    </owl:NamedIndividual>
    


    <!-- http://purl.obolibrary.org/obo/GAZ_00076124 -->

    <owl:NamedIndividual rdf:about="http://purl.obolibrary.org/obo/GAZ_00076124">
        <obo:RO_0001025 rdf:resource="http://purl.obolibrary.org/obo/GAZ_00032845"/>
        <obo:IAO_0000115>A local municipality located in the Western Cape Province of South Africa.</obo:IAO_0000115>
        <oboInOwl:hasOBONamespace>GAZ</oboInOwl:hasOBONamespace>
        <oboInOwl:id>GAZ:00076124</oboInOwl:id>
        <rdfs:label>Cape Agulhas Local Municipality</rdfs:label>
    </owl:NamedIndividual>
    


    <!-- http://purl.obolibrary.org/obo/GAZ_00076125 -->

    <owl:NamedIndividual rdf:about="http://purl.obolibrary.org/obo/GAZ_00076125">
        <obo:RO_0001025 rdf:resource="http://purl.obolibrary.org/obo/GAZ_00032845"/>
        <obo:IAO_0000115>A local municipality located in the Western Cape Province of South Africa.</obo:IAO_0000115>
        <oboInOwl:hasOBONamespace>GAZ</oboInOwl:hasOBONamespace>
        <oboInOwl:id>GAZ:00076125</oboInOwl:id>
        <rdfs:label>Swellendam Local Municipality</rdfs:label>
    </owl:NamedIndividual>
    


    <!-- http://purl.obolibrary.org/obo/GAZ_00076126 -->

    <owl:NamedIndividual rdf:about="http://purl.obolibrary.org/obo/GAZ_00076126">
        <obo:RO_0001025 rdf:resource="http://purl.obolibrary.org/obo/GAZ_00032845"/>
        <obo:IAO_0000115>A local municipality located in the Western Cape Province of South Africa.</obo:IAO_0000115>
        <oboInOwl:hasOBONamespace>GAZ</oboInOwl:hasOBONamespace>
        <oboInOwl:id>GAZ:00076126</oboInOwl:id>
        <rdfs:label>Theewaterskloof Local Municipality</rdfs:label>
    </owl:NamedIndividual>
    


    <!-- http://purl.obolibrary.org/obo/GAZ_00076127 -->

    <owl:NamedIndividual rdf:about="http://purl.obolibrary.org/obo/GAZ_00076127">
        <obo:RO_0001025 rdf:resource="http://purl.obolibrary.org/obo/GAZ_00012792"/>
        <obo:IAO_0000115>A local municipality located in the Western Cape Province of South Africa.</obo:IAO_0000115>
        <oboInOwl:hasOBONamespace>GAZ</oboInOwl:hasOBONamespace>
        <oboInOwl:id>GAZ:00076127</oboInOwl:id>
        <rdfs:label>Hessequa Local Municipality</rdfs:label>
    </owl:NamedIndividual>
    


    <!-- http://purl.obolibrary.org/obo/GAZ_00076128 -->

    <owl:NamedIndividual rdf:about="http://purl.obolibrary.org/obo/GAZ_00076128">
        <obo:RO_0001025 rdf:resource="http://purl.obolibrary.org/obo/GAZ_00012792"/>
        <obo:IAO_0000115>A local municipality located in the Western Cape Province of South Africa.</obo:IAO_0000115>
        <oboInOwl:hasOBONamespace>GAZ</oboInOwl:hasOBONamespace>
        <oboInOwl:id>GAZ:00076128</oboInOwl:id>
        <rdfs:label>George Local Municipality</rdfs:label>
    </owl:NamedIndividual>
    


    <!-- http://purl.obolibrary.org/obo/GAZ_00076129 -->

    <owl:NamedIndividual rdf:about="http://purl.obolibrary.org/obo/GAZ_00076129">
        <obo:RO_0001025 rdf:resource="http://purl.obolibrary.org/obo/GAZ_00012792"/>
        <obo:IAO_0000115>A local municipality located in the Western Cape Province of South Africa.</obo:IAO_0000115>
        <oboInOwl:hasOBONamespace>GAZ</oboInOwl:hasOBONamespace>
        <oboInOwl:id>GAZ:00076129</oboInOwl:id>
        <rdfs:label>Kannaland Local Municipality</rdfs:label>
    </owl:NamedIndividual>
    


    <!-- http://purl.obolibrary.org/obo/GAZ_00076130 -->

    <owl:NamedIndividual rdf:about="http://purl.obolibrary.org/obo/GAZ_00076130">
        <obo:RO_0001025 rdf:resource="http://purl.obolibrary.org/obo/GAZ_00012792"/>
        <obo:IAO_0000115>A local municipality located in the Western Cape Province of South Africa.</obo:IAO_0000115>
        <oboInOwl:hasOBONamespace>GAZ</oboInOwl:hasOBONamespace>
        <oboInOwl:id>GAZ:00076130</oboInOwl:id>
        <rdfs:label>Mossel Bay Local Municipality</rdfs:label>
    </owl:NamedIndividual>
    


    <!-- http://purl.obolibrary.org/obo/GAZ_00076131 -->

    <owl:NamedIndividual rdf:about="http://purl.obolibrary.org/obo/GAZ_00076131">
        <obo:RO_0001025 rdf:resource="http://purl.obolibrary.org/obo/GAZ_00012792"/>
        <obo:IAO_0000115>A local municipality located in the Western Cape Province of South Africa.</obo:IAO_0000115>
        <oboInOwl:hasOBONamespace>GAZ</oboInOwl:hasOBONamespace>
        <oboInOwl:id>GAZ:00076131</oboInOwl:id>
        <rdfs:label>Bitou Local Municipality</rdfs:label>
    </owl:NamedIndividual>
    


    <!-- http://purl.obolibrary.org/obo/GAZ_00076132 -->

    <owl:NamedIndividual rdf:about="http://purl.obolibrary.org/obo/GAZ_00076132">
        <obo:RO_0001025 rdf:resource="http://purl.obolibrary.org/obo/GAZ_00032855"/>
        <obo:IAO_0000115>A local municipality located in the Western Cape Province of South Africa.</obo:IAO_0000115>
        <oboInOwl:hasOBONamespace>GAZ</oboInOwl:hasOBONamespace>
        <oboInOwl:id>GAZ:00076132</oboInOwl:id>
        <rdfs:label>Prince Albert Local Municipality</rdfs:label>
    </owl:NamedIndividual>
    


    <!-- http://purl.obolibrary.org/obo/GAZ_00076133 -->

    <owl:NamedIndividual rdf:about="http://purl.obolibrary.org/obo/GAZ_00076133">
        <obo:RO_0001025 rdf:resource="http://purl.obolibrary.org/obo/GAZ_00032855"/>
        <obo:IAO_0000115>A local municipality located in the Western Cape Province of South Africa.</obo:IAO_0000115>
        <oboInOwl:hasOBONamespace>GAZ</oboInOwl:hasOBONamespace>
        <oboInOwl:id>GAZ:00076133</oboInOwl:id>
        <rdfs:label>Laingsburg Local Municipality</rdfs:label>
    </owl:NamedIndividual>
    


    <!-- http://purl.obolibrary.org/obo/GAZ_00076134 -->

    <owl:NamedIndividual rdf:about="http://purl.obolibrary.org/obo/GAZ_00076134">
        <obo:RO_0001025 rdf:resource="http://purl.obolibrary.org/obo/GAZ_00032855"/>
        <obo:IAO_0000115>A local municipality located in the Western Cape Province of South Africa.</obo:IAO_0000115>
        <oboInOwl:hasOBONamespace>GAZ</oboInOwl:hasOBONamespace>
        <oboInOwl:id>GAZ:00076134</oboInOwl:id>
        <rdfs:label>Beaufort West Local Municipality</rdfs:label>
    </owl:NamedIndividual>
    


    <!-- http://purl.obolibrary.org/obo/GAZ_00076135 -->

    <owl:NamedIndividual rdf:about="http://purl.obolibrary.org/obo/GAZ_00076135">
        <obo:RO_0001025 rdf:resource="http://purl.obolibrary.org/obo/GAZ_00032856"/>
        <obo:IAO_0000115>Three District Management Areas in the West Coast District Municipality.</obo:IAO_0000115>
        <oboInOwl:hasOBONamespace>GAZ</oboInOwl:hasOBONamespace>
        <oboInOwl:id>GAZ:00076135</oboInOwl:id>
        <rdfs:label>West Coast District Management Areas</rdfs:label>
    </owl:NamedIndividual>
    


    <!-- http://purl.obolibrary.org/obo/GAZ_00076136 -->

    <owl:NamedIndividual rdf:about="http://purl.obolibrary.org/obo/GAZ_00076136">
        <obo:RO_0001025 rdf:resource="http://purl.obolibrary.org/obo/GAZ_00076138"/>
        <obo:IAO_0000115>A mountain range is part of the Cape Fold Belt in the Western Cape, South Africa. The range forms a barrier between the Cape Town metropolitan area and the southern Overberg coast.</obo:IAO_0000115>
        <oboInOwl:hasOBONamespace>GAZ</oboInOwl:hasOBONamespace>
        <oboInOwl:id>GAZ:00076136</oboInOwl:id>
        <rdfs:label>Hottentots-Holland Mountains</rdfs:label>
    </owl:NamedIndividual>
    


    <!-- http://purl.obolibrary.org/obo/GAZ_00076137 -->

    <owl:NamedIndividual rdf:about="http://purl.obolibrary.org/obo/GAZ_00076137">
        <obo:RO_0001025 rdf:resource="http://purl.obolibrary.org/obo/GAZ_00076138"/>
        <obo:IAO_0000115>A mountain range located near Clanwilliam, approximately 300 km north of Cape Town, South Africa. The Cederberg mountains extend about 50 km north-south by 20 km east-west. They are bordered on the west by the Sandveld, the north by the Pakhuis Mountains, the East by the Springbok flats and the south by the Kouebokkeveld mountains and the Skurweberge.</obo:IAO_0000115>
        <oboInOwl:hasOBONamespace>GAZ</oboInOwl:hasOBONamespace>
        <oboInOwl:id>GAZ:00076137</oboInOwl:id>
        <rdfs:label>Cederberg</rdfs:label>
    </owl:NamedIndividual>
    


    <!-- http://purl.obolibrary.org/obo/GAZ_00076138 -->

    <owl:NamedIndividual rdf:about="http://purl.obolibrary.org/obo/GAZ_00076138">
        <obo:RO_0001025 rdf:resource="http://purl.obolibrary.org/obo/GAZ_00002817"/>
        <obo:IAO_0000115>The folded sedimentary sequence of rocks in the southwestern corner of South Africa.</obo:IAO_0000115>
        <oboInOwl:hasOBONamespace>GAZ</oboInOwl:hasOBONamespace>
        <oboInOwl:id>GAZ:00076138</oboInOwl:id>
        <rdfs:label>Cape Fold Belt</rdfs:label>
    </owl:NamedIndividual>
    


    <!-- http://purl.obolibrary.org/obo/GAZ_00076139 -->

    <owl:NamedIndividual rdf:about="http://purl.obolibrary.org/obo/GAZ_00076139">
        <obo:RO_0001025 rdf:resource="http://purl.obolibrary.org/obo/GAZ_00076138"/>
        <oboInOwl:hasOBONamespace>GAZ</oboInOwl:hasOBONamespace>
        <oboInOwl:id>GAZ:00076139</oboInOwl:id>
        <rdfs:label>Olifants River Mountains</rdfs:label>
    </owl:NamedIndividual>
    


    <!-- http://purl.obolibrary.org/obo/GAZ_00076140 -->

    <owl:NamedIndividual rdf:about="http://purl.obolibrary.org/obo/GAZ_00076140">
        <obo:RO_0001025 rdf:resource="http://purl.obolibrary.org/obo/GAZ_00076138"/>
        <oboInOwl:hasOBONamespace>GAZ</oboInOwl:hasOBONamespace>
        <oboInOwl:id>GAZ:00076140</oboInOwl:id>
        <rdfs:label>Piketberg</rdfs:label>
    </owl:NamedIndividual>
    


    <!-- http://purl.obolibrary.org/obo/GAZ_00076141 -->

    <owl:NamedIndividual rdf:about="http://purl.obolibrary.org/obo/GAZ_00076141">
        <obo:RO_0001025 rdf:resource="http://purl.obolibrary.org/obo/GAZ_00076138"/>
        <obo:IAO_0000115>A mountain range located in the Western Cape province of South Africa and are part of the Cape Fold Belt. They rise to a maximum height of 2077m just north of the town of Tulbagh as Grootwinterhoekpiek.</obo:IAO_0000115>
        <oboInOwl:hasOBONamespace>GAZ</oboInOwl:hasOBONamespace>
        <oboInOwl:id>GAZ:00076141</oboInOwl:id>
        <rdfs:label>Winterhoekberge</rdfs:label>
    </owl:NamedIndividual>
    


    <!-- http://purl.obolibrary.org/obo/GAZ_00076142 -->

    <owl:NamedIndividual rdf:about="http://purl.obolibrary.org/obo/GAZ_00076142">
        <obo:RO_0001025 rdf:resource="http://purl.obolibrary.org/obo/GAZ_00076138"/>
        <oboInOwl:hasOBONamespace>GAZ</oboInOwl:hasOBONamespace>
        <oboInOwl:id>GAZ:00076142</oboInOwl:id>
        <rdfs:label>Skurweberge</rdfs:label>
    </owl:NamedIndividual>
    


    <!-- http://purl.obolibrary.org/obo/GAZ_00076143 -->

    <owl:NamedIndividual rdf:about="http://purl.obolibrary.org/obo/GAZ_00076143">
        <obo:RO_0001025 rdf:resource="http://purl.obolibrary.org/obo/GAZ_00076138"/>
        <obo:IAO_0000115>A mountain range located 120 km north-east of Cape Town. They form part of a large anticline in the Cape Fold Belt mountain system and form a north-east, south-west trending mountain system forming the core of the Cape Syntaxis between the towns of Worcester and De Doorns.</obo:IAO_0000115>
        <oboInOwl:hasOBONamespace>GAZ</oboInOwl:hasOBONamespace>
        <oboInOwl:id>GAZ:00076143</oboInOwl:id>
        <rdfs:label>Hex River Mountains</rdfs:label>
    </owl:NamedIndividual>
    


    <!-- http://purl.obolibrary.org/obo/GAZ_00076144 -->

    <owl:NamedIndividual rdf:about="http://purl.obolibrary.org/obo/GAZ_00076144">
        <obo:RO_0001025 rdf:resource="http://purl.obolibrary.org/obo/GAZ_00076138"/>
        <obo:IAO_0000115>Mountains located between Paarl and Worcester in the south-west of South Africa, 70 km to the north-east of the provincial capital of Cape Town.</obo:IAO_0000115>
        <oboInOwl:hasOBONamespace>GAZ</oboInOwl:hasOBONamespace>
        <oboInOwl:id>GAZ:00076144</oboInOwl:id>
        <rdfs:label>Du Toits Mountains</rdfs:label>
    </owl:NamedIndividual>
    


    <!-- http://purl.obolibrary.org/obo/GAZ_00076145 -->

    <owl:NamedIndividual rdf:about="http://purl.obolibrary.org/obo/GAZ_00076145">
        <obo:RO_0001025 rdf:resource="http://purl.obolibrary.org/obo/GAZ_00076138"/>
        <obo:IAO_0000115>A mountain range that is part of the Cape Fold Belt and are in the Western Cape province of South Africa.</obo:IAO_0000115>
        <oboInOwl:hasOBONamespace>GAZ</oboInOwl:hasOBONamespace>
        <oboInOwl:id>GAZ:00076145</oboInOwl:id>
        <rdfs:label>Drakenstein Mountains</rdfs:label>
    </owl:NamedIndividual>
    


    <!-- http://purl.obolibrary.org/obo/GAZ_00076146 -->

    <owl:NamedIndividual rdf:about="http://purl.obolibrary.org/obo/GAZ_00076146">
        <obo:RO_0001025 rdf:resource="http://purl.obolibrary.org/obo/GAZ_00076145"/>
        <obo:IAO_0000115>A subrange of the Drakenstein Mountains located south of Franschhoek and Stellenbosch, with Victoria Peak (1590m) as its highest point. It is traversed by no mountain passes, but contains the Hottentots-Holland Nature Reserve.</obo:IAO_0000115>
        <oboInOwl:hasOBONamespace>GAZ</oboInOwl:hasOBONamespace>
        <oboInOwl:id>GAZ:00076146</oboInOwl:id>
        <rdfs:label>Groot Drakenstein</rdfs:label>
    </owl:NamedIndividual>
    


    <!-- http://purl.obolibrary.org/obo/GAZ_00076147 -->

    <owl:NamedIndividual rdf:about="http://purl.obolibrary.org/obo/GAZ_00076147">
        <obo:RO_0001025 rdf:resource="http://purl.obolibrary.org/obo/GAZ_00076145"/>
        <obo:IAO_0000115>A subrange of the Drakenstein Mountains located just to the east of Paarl being punctuated by the Huguenot Tunnel on the N1 highway and Du Toitskloof Pass (820m) as the R101 route.</obo:IAO_0000115>
        <oboInOwl:hasOBONamespace>GAZ</oboInOwl:hasOBONamespace>
        <oboInOwl:id>GAZ:00076147</oboInOwl:id>
        <rdfs:label>Klein Drakenstein</rdfs:label>
    </owl:NamedIndividual>
    


    <!-- http://purl.obolibrary.org/obo/GAZ_00076148 -->

    <owl:NamedIndividual rdf:about="http://purl.obolibrary.org/obo/GAZ_00076148">
        <obo:RO_0001025 rdf:resource="http://purl.obolibrary.org/obo/GAZ_00076138"/>
        <obo:IAO_0000115>Part of the Cape Fold Belt in the Western Cape province of South Africa and is located between the towns of Stellenbosch, Paarl and Franschhoek, forming a prominent 1399 m high mountain, as it is detached from the other ranges in the winelands region.</obo:IAO_0000115>
        <oboInOwl:hasOBONamespace>GAZ</oboInOwl:hasOBONamespace>
        <oboInOwl:id>GAZ:00076148</oboInOwl:id>
        <rdfs:label>Simonsberg</rdfs:label>
    </owl:NamedIndividual>
    


    <!-- http://purl.obolibrary.org/obo/GAZ_00076149 -->

    <owl:NamedIndividual rdf:about="http://purl.obolibrary.org/obo/GAZ_00076149">
        <rdf:type rdf:resource="http://purl.obolibrary.org/obo/ENVO_00000106"/>
        <obo:RO_0001025 rdf:resource="http://purl.obolibrary.org/obo/GAZ_00076138"/>
        <obo:IAO_0000115>A range of mountains along the False Bay coast in the Western Cape of South Africa. They form part of the Cape Fold Belt and start south of Grabouw and form a steep coastal range to Kleinmond.</obo:IAO_0000115>
        <oboInOwl:hasOBONamespace>GAZ</oboInOwl:hasOBONamespace>
        <oboInOwl:id>GAZ:00076149</oboInOwl:id>
        <rdfs:label>Kogelberg</rdfs:label>
    </owl:NamedIndividual>
    


    <!-- http://purl.obolibrary.org/obo/GAZ_00076150 -->

    <owl:NamedIndividual rdf:about="http://purl.obolibrary.org/obo/GAZ_00076150">
        <obo:RO_0001025 rdf:resource="http://purl.obolibrary.org/obo/GAZ_00076138"/>
        <oboInOwl:hasOBONamespace>GAZ</oboInOwl:hasOBONamespace>
        <oboInOwl:id>GAZ:00076150</oboInOwl:id>
        <rdfs:label>Stettynsberge</rdfs:label>
    </owl:NamedIndividual>
    


    <!-- http://purl.obolibrary.org/obo/GAZ_00076151 -->

    <owl:NamedIndividual rdf:about="http://purl.obolibrary.org/obo/GAZ_00076151">
        <obo:RO_0001025 rdf:resource="http://purl.obolibrary.org/obo/GAZ_00076138"/>
        <obo:IAO_0000115>A mountain range that runs in a generally east-west direction and is approximately 170 km long. The Langeberg&apos;s most westerly point is located 35 km west of the town of Swellendam; the range ends some 30 km north-east of Riversdale in the east. The open plains of the Little Karoo border the north of the mountain range, while to the south lies the Agulhas Plain and the Overberg wheatbelt.</obo:IAO_0000115>
        <oboInOwl:hasOBONamespace>GAZ</oboInOwl:hasOBONamespace>
        <oboInOwl:id>GAZ:00076151</oboInOwl:id>
        <rdfs:label>Langeberg Mountain Range</rdfs:label>
    </owl:NamedIndividual>
    


    <!-- http://purl.obolibrary.org/obo/GAZ_00076152 -->

    <owl:NamedIndividual rdf:about="http://purl.obolibrary.org/obo/GAZ_00076152">
        <obo:RO_0001025 rdf:resource="http://purl.obolibrary.org/obo/GAZ_00076138"/>
        <obo:IAO_0000115>A mountain range in the Cape Fold Belt of the Western Cape province of South Africa. They run east to west from Riviersonderend to Villiersdorp, separating the Breede River Valley from the Overberg region.</obo:IAO_0000115>
        <oboInOwl:hasOBONamespace>GAZ</oboInOwl:hasOBONamespace>
        <oboInOwl:id>GAZ:00076152</oboInOwl:id>
        <rdfs:label>Riviersonderend Mountains</rdfs:label>
    </owl:NamedIndividual>
    


    <!-- http://purl.obolibrary.org/obo/GAZ_00076153 -->

    <owl:NamedIndividual rdf:about="http://purl.obolibrary.org/obo/GAZ_00076153">
        <obo:RO_0001025 rdf:resource="http://purl.obolibrary.org/obo/GAZ_00076138"/>
        <obo:IAO_0000115>A mountain range of mountains in the Cape Fold Belt of the Western Cape province of South Africa.</obo:IAO_0000115>
        <oboInOwl:hasOBONamespace>GAZ</oboInOwl:hasOBONamespace>
        <oboInOwl:id>GAZ:00076153</oboInOwl:id>
        <rdfs:label>Kleinrivier Mountains</rdfs:label>
    </owl:NamedIndividual>
    


    <!-- http://purl.obolibrary.org/obo/GAZ_00076154 -->

    <owl:NamedIndividual rdf:about="http://purl.obolibrary.org/obo/GAZ_00076154">
        <obo:RO_0001025 rdf:resource="http://purl.obolibrary.org/obo/GAZ_00076153"/>
        <oboInOwl:hasOBONamespace>GAZ</oboInOwl:hasOBONamespace>
        <oboInOwl:id>GAZ:00076154</oboInOwl:id>
        <rdfs:label>Babilonstoring Mountains</rdfs:label>
    </owl:NamedIndividual>
    


    <!-- http://purl.obolibrary.org/obo/GAZ_00076155 -->

    <owl:NamedIndividual rdf:about="http://purl.obolibrary.org/obo/GAZ_00076155">
        <obo:RO_0001025 rdf:resource="http://purl.obolibrary.org/obo/GAZ_00076138"/>
        <oboInOwl:hasOBONamespace>GAZ</oboInOwl:hasOBONamespace>
        <oboInOwl:id>GAZ:00076155</oboInOwl:id>
        <rdfs:label>Witteberge</rdfs:label>
    </owl:NamedIndividual>
    


    <!-- http://purl.obolibrary.org/obo/GAZ_00076156 -->

    <owl:NamedIndividual rdf:about="http://purl.obolibrary.org/obo/GAZ_00076156">
        <obo:RO_0001025 rdf:resource="http://purl.obolibrary.org/obo/GAZ_00076138"/>
        <obo:IAO_0000115>A mountain range that runs roughly east-west along the northern edge of the semi-arid area called the Little Karoo in the Western Cape province of South Africa. To the north of the range lies the other large semi-arid area in South Africa, the Great Karoo.</obo:IAO_0000115>
        <oboInOwl:hasOBONamespace>GAZ</oboInOwl:hasOBONamespace>
        <oboInOwl:id>GAZ:00076156</oboInOwl:id>
        <rdfs:label>Swartberg</rdfs:label>
    </owl:NamedIndividual>
    


    <!-- http://purl.obolibrary.org/obo/GAZ_00076157 -->

    <owl:NamedIndividual rdf:about="http://purl.obolibrary.org/obo/GAZ_00076157">
        <obo:RO_0001025 rdf:resource="http://purl.obolibrary.org/obo/GAZ_00001094"/>
        <obo:IAO_0000115>A semi-desert region of South Africa. It has two main sub-regions - the Great Karoo in the north and the Little Karoo in the south. The &apos;High&apos; Karoo is one of the distinct physiographic provinces of the larger South African Platform division.</obo:IAO_0000115>
        <oboInOwl:hasOBONamespace>GAZ</oboInOwl:hasOBONamespace>
        <oboInOwl:id>GAZ:00076157</oboInOwl:id>
        <rdfs:label>Karoo</rdfs:label>
    </owl:NamedIndividual>
    


    <!-- http://purl.obolibrary.org/obo/GAZ_00076158 -->

    <owl:NamedIndividual rdf:about="http://purl.obolibrary.org/obo/GAZ_00076158">
        <obo:RO_0001025 rdf:resource="http://purl.obolibrary.org/obo/GAZ_00076157"/>
        <obo:IAO_0000115>A fertile valley (bounded on the north by the Swartberg, and on the south by the Langeberg and Outeniqua mountains). Although the boundaries of the region are not strictly defined, most people consider the western limit of the Little Karoo to be in the region of Barrydale and the eastern extremity around Uniondale.</obo:IAO_0000115>
        <oboInOwl:hasOBONamespace>GAZ</oboInOwl:hasOBONamespace>
        <oboInOwl:id>GAZ:00076158</oboInOwl:id>
        <rdfs:label>Little Karoo</rdfs:label>
    </owl:NamedIndividual>
    


    <!-- http://purl.obolibrary.org/obo/GAZ_00076159 -->

    <owl:NamedIndividual rdf:about="http://purl.obolibrary.org/obo/GAZ_00076159">
        <obo:RO_0001025 rdf:resource="http://purl.obolibrary.org/obo/GAZ_00076157"/>
        <oboInOwl:hasOBONamespace>GAZ</oboInOwl:hasOBONamespace>
        <oboInOwl:id>GAZ:00076159</oboInOwl:id>
        <rdfs:label>Great Karoo</rdfs:label>
    </owl:NamedIndividual>
    


    <!-- http://purl.obolibrary.org/obo/GAZ_00076160 -->

    <owl:NamedIndividual rdf:about="http://purl.obolibrary.org/obo/GAZ_00076160">
        <obo:RO_0001025 rdf:resource="http://purl.obolibrary.org/obo/GAZ_00076156"/>
        <obo:IAO_0000115>The W subrange of the Swartberg, the dividing line between it and the Greater Swartberg being the Gouritz river.</obo:IAO_0000115>
        <oboInOwl:hasOBONamespace>GAZ</oboInOwl:hasOBONamespace>
        <oboInOwl:id>GAZ:00076160</oboInOwl:id>
        <rdfs:label>Small Swartberg Mountains</rdfs:label>
    </owl:NamedIndividual>
    


    <!-- http://purl.obolibrary.org/obo/GAZ_00076161 -->

    <owl:NamedIndividual rdf:about="http://purl.obolibrary.org/obo/GAZ_00076161">
        <obo:RO_0001025 rdf:resource="http://purl.obolibrary.org/obo/GAZ_00076156"/>
        <obo:IAO_0000115>The E subrange of the Swartberg, the dividing line between it and the Small Swartberg being the Gouritz river.</obo:IAO_0000115>
        <oboInOwl:hasOBONamespace>GAZ</oboInOwl:hasOBONamespace>
        <oboInOwl:id>GAZ:00076161</oboInOwl:id>
        <rdfs:label>Greater Swartberg Mountains</rdfs:label>
    </owl:NamedIndividual>
    


    <!-- http://purl.obolibrary.org/obo/GAZ_00076162 -->

    <owl:NamedIndividual rdf:about="http://purl.obolibrary.org/obo/GAZ_00076162">
        <obo:RO_0001025 rdf:resource="http://purl.obolibrary.org/obo/GAZ_00076138"/>
        <obo:IAO_0000115>A mountain range located in the Western Cape Province of South Africa. It is traversed by the Montagu Pass and the Outeniqua Pass. The Outeniqua range rises from the Indian Ocean coastal plain, north of the town of Mossel Bay. It continues for about 100 km to the east before ending at the Keurbooms River Valley, which enters the ocean at Plettenberg Bay. The range runs parallel to the Swartberg Mountain Range.</obo:IAO_0000115>
        <oboInOwl:hasOBONamespace>GAZ</oboInOwl:hasOBONamespace>
        <oboInOwl:id>GAZ:00076162</oboInOwl:id>
        <rdfs:label>Outeniqua Mountain Range</rdfs:label>
    </owl:NamedIndividual>
    


    <!-- http://purl.obolibrary.org/obo/GAZ_00076163 -->

    <owl:NamedIndividual rdf:about="http://purl.obolibrary.org/obo/GAZ_00076163">
        <obo:RO_0001025 rdf:resource="http://purl.obolibrary.org/obo/GAZ_00076138"/>
        <obo:IAO_0000115>A short range within the Cape Fold Belt in the Western Cape of South Africa. They form a link between the Outeniqua and Tsitsikamma Mountains to the north of Plettenberg Bay in the Garden Route region. They stretch from Prince Alfred&apos;s Pass in the west to just north of Nature&apos;s Valley and south of Joubertina.</obo:IAO_0000115>
        <oboInOwl:hasOBONamespace>GAZ</oboInOwl:hasOBONamespace>
        <oboInOwl:id>GAZ:00076163</oboInOwl:id>
        <rdfs:label>Langkloof Mountains</rdfs:label>
    </owl:NamedIndividual>
    


    <!-- http://purl.obolibrary.org/obo/GAZ_00076164 -->

    <owl:NamedIndividual rdf:about="http://purl.obolibrary.org/obo/GAZ_00076164">
        <obo:RO_0001025 rdf:resource="http://purl.obolibrary.org/obo/GAZ_00076138"/>
        <oboInOwl:hasOBONamespace>GAZ</oboInOwl:hasOBONamespace>
        <oboInOwl:id>GAZ:00076164</oboInOwl:id>
        <rdfs:label>Kouga Mountains</rdfs:label>
    </owl:NamedIndividual>
    


    <!-- http://purl.obolibrary.org/obo/GAZ_00076165 -->

    <owl:NamedIndividual rdf:about="http://purl.obolibrary.org/obo/GAZ_00076165">
        <obo:RO_0001025 rdf:resource="http://purl.obolibrary.org/obo/GAZ_00076138"/>
        <oboInOwl:hasOBONamespace>GAZ</oboInOwl:hasOBONamespace>
        <oboInOwl:id>GAZ:00076165</oboInOwl:id>
        <rdfs:label>Baviaanskloof Mountains</rdfs:label>
    </owl:NamedIndividual>
    


    <!-- http://purl.obolibrary.org/obo/GAZ_00076167 -->

    <owl:NamedIndividual rdf:about="http://purl.obolibrary.org/obo/GAZ_00076167">
        <obo:RO_0001025 rdf:resource="http://purl.obolibrary.org/obo/GAZ_00076138"/>
        <oboInOwl:hasOBONamespace>GAZ</oboInOwl:hasOBONamespace>
        <oboInOwl:id>GAZ:00076167</oboInOwl:id>
        <rdfs:label>Zuurberge</rdfs:label>
    </owl:NamedIndividual>
    


    <!-- http://purl.obolibrary.org/obo/GAZ_00076169 -->

    <owl:NamedIndividual rdf:about="http://purl.obolibrary.org/obo/GAZ_00076169">
        <obo:RO_0001025 rdf:resource="http://purl.obolibrary.org/obo/GAZ_00012790"/>
        <oboInOwl:hasOBONamespace>GAZ</oboInOwl:hasOBONamespace>
        <oboInOwl:id>GAZ:00076169</oboInOwl:id>
        <rdfs:label>Breede River District Management Area</rdfs:label>
    </owl:NamedIndividual>
    


    <!-- http://purl.obolibrary.org/obo/GAZ_00076170 -->

    <owl:NamedIndividual rdf:about="http://purl.obolibrary.org/obo/GAZ_00076170">
        <obo:RO_0001025 rdf:resource="http://purl.obolibrary.org/obo/GAZ_00032855"/>
        <oboInOwl:hasOBONamespace>GAZ</oboInOwl:hasOBONamespace>
        <oboInOwl:id>GAZ:00076170</oboInOwl:id>
        <rdfs:label>Central Karoo District Management Area</rdfs:label>
    </owl:NamedIndividual>
    


    <!-- http://purl.obolibrary.org/obo/GAZ_00076171 -->

    <owl:NamedIndividual rdf:about="http://purl.obolibrary.org/obo/GAZ_00076171">
        <obo:RO_0001025 rdf:resource="http://purl.obolibrary.org/obo/GAZ_00012792"/>
        <oboInOwl:hasOBONamespace>GAZ</oboInOwl:hasOBONamespace>
        <oboInOwl:id>GAZ:00076171</oboInOwl:id>
        <rdfs:label>South Cape District Management Area</rdfs:label>
    </owl:NamedIndividual>
    


    <!-- http://purl.obolibrary.org/obo/GAZ_00076172 -->

    <owl:NamedIndividual rdf:about="http://purl.obolibrary.org/obo/GAZ_00076172">
        <obo:RO_0001025 rdf:resource="http://purl.obolibrary.org/obo/GAZ_00032845"/>
        <oboInOwl:hasOBONamespace>GAZ</oboInOwl:hasOBONamespace>
        <oboInOwl:id>GAZ:00076172</oboInOwl:id>
        <rdfs:label>Overberg District Management Area</rdfs:label>
    </owl:NamedIndividual>
    


    <!-- http://purl.obolibrary.org/obo/GAZ_00076173 -->

    <owl:NamedIndividual rdf:about="http://purl.obolibrary.org/obo/GAZ_00076173">
        <obo:RO_0001025 rdf:resource="http://purl.obolibrary.org/obo/GAZ_00032873"/>
        <obo:IAO_0000115>A District Management Area in Siyanda District Municipality.</obo:IAO_0000115>
        <oboInOwl:hasOBONamespace>GAZ</oboInOwl:hasOBONamespace>
        <oboInOwl:id>GAZ:00076173</oboInOwl:id>
        <rdfs:label>Benede Oranje District Management Area</rdfs:label>
    </owl:NamedIndividual>
    


    <!-- http://purl.obolibrary.org/obo/GAZ_00076174 -->

    <owl:NamedIndividual rdf:about="http://purl.obolibrary.org/obo/GAZ_00076174">
        <obo:RO_0001025 rdf:resource="http://purl.obolibrary.org/obo/GAZ_00032869"/>
        <obo:IAO_0000115>A District Management Area in North Cape Province.</obo:IAO_0000115>
        <oboInOwl:hasOBONamespace>GAZ</oboInOwl:hasOBONamespace>
        <oboInOwl:id>GAZ:00076174</oboInOwl:id>
        <rdfs:label>Kalahari District Management Area</rdfs:label>
    </owl:NamedIndividual>
    


    <!-- http://purl.obolibrary.org/obo/GAZ_00076175 -->

    <owl:NamedIndividual rdf:about="http://purl.obolibrary.org/obo/GAZ_00076175">
        <obo:RO_0001025 rdf:resource="http://purl.obolibrary.org/obo/GAZ_00032886"/>
        <obo:IAO_0000115>A nature reserve and District Management Area in Nkangala District Municipality.</obo:IAO_0000115>
        <oboInOwl:hasOBONamespace>GAZ</oboInOwl:hasOBONamespace>
        <oboInOwl:id>GAZ:00076175</oboInOwl:id>
        <rdfs:label>Mdala Nature Reserve</rdfs:label>
    </owl:NamedIndividual>
    


    <!-- http://purl.obolibrary.org/obo/GAZ_00076176 -->

    <owl:NamedIndividual rdf:about="http://purl.obolibrary.org/obo/GAZ_00076176">
        <obo:RO_0001025 rdf:resource="http://purl.obolibrary.org/obo/GAZ_00032887"/>
        <obo:IAO_0000115>A District Management Area in Ehlanzeni District Municipality.</obo:IAO_0000115>
        <oboInOwl:hasOBONamespace>GAZ</oboInOwl:hasOBONamespace>
        <oboInOwl:id>GAZ:00076176</oboInOwl:id>
        <rdfs:label>Lowveld District Management Area</rdfs:label>
    </owl:NamedIndividual>
    


    <!-- http://purl.obolibrary.org/obo/GAZ_00076177 -->

    <owl:NamedIndividual rdf:about="http://purl.obolibrary.org/obo/GAZ_00076177">
        <obo:RO_0001025 rdf:resource="http://purl.obolibrary.org/obo/GAZ_00012785"/>
        <obo:IAO_0000115>A District Management Area in the West Rand District Municipality.</obo:IAO_0000115>
        <oboInOwl:hasOBONamespace>GAZ</oboInOwl:hasOBONamespace>
        <oboInOwl:id>GAZ:00076177</oboInOwl:id>
        <rdfs:label>West Rand District Management Area</rdfs:label>
    </owl:NamedIndividual>
    


    <!-- http://purl.obolibrary.org/obo/GAZ_00076178 -->

    <owl:NamedIndividual rdf:about="http://purl.obolibrary.org/obo/GAZ_00076178">
        <obo:RO_0001025 rdf:resource="http://purl.obolibrary.org/obo/GAZ_00032858"/>
        <obo:IAO_0000115>A District Management Area in Cacadu District Municipality.</obo:IAO_0000115>
        <oboInOwl:hasOBONamespace>GAZ</oboInOwl:hasOBONamespace>
        <oboInOwl:id>GAZ:00076178</oboInOwl:id>
        <rdfs:label>Aberdeen Plain District Management Area</rdfs:label>
    </owl:NamedIndividual>
    


    <!-- http://purl.obolibrary.org/obo/GAZ_00076179 -->

    <owl:NamedIndividual rdf:about="http://purl.obolibrary.org/obo/GAZ_00076179">
        <obo:RO_0001025 rdf:resource="http://purl.obolibrary.org/obo/GAZ_00032857"/>
        <obo:IAO_0000115>A national park in the Eastern Cape Province of South Africa proclaimed in 1937-07.</obo:IAO_0000115>
        <oboInOwl:hasOBONamespace>GAZ</oboInOwl:hasOBONamespace>
        <oboInOwl:id>GAZ:00076179</oboInOwl:id>
        <rdfs:label>Mountain Zebra National Park</rdfs:label>
    </owl:NamedIndividual>
    


    <!-- http://purl.obolibrary.org/obo/GAZ_00076180 -->

    <owl:NamedIndividual rdf:about="http://purl.obolibrary.org/obo/GAZ_00076180">
        <obo:RO_0001025 rdf:resource="http://purl.obolibrary.org/obo/GAZ_00075955"/>
        <obo:IAO_0000115>A national park situated close to Port Elizabeth in South Africa.</obo:IAO_0000115>
        <oboInOwl:hasOBONamespace>GAZ</oboInOwl:hasOBONamespace>
        <oboInOwl:id>GAZ:00076180</oboInOwl:id>
        <rdfs:label>Addo Elephant National Park</rdfs:label>
    </owl:NamedIndividual>
    


    <!-- http://purl.obolibrary.org/obo/GAZ_00076181 -->

    <owl:NamedIndividual rdf:about="http://purl.obolibrary.org/obo/GAZ_00076181">
        <obo:RO_0001025 rdf:resource="http://purl.obolibrary.org/obo/GAZ_00002815"/>
        <obo:IAO_0000115>A conservation park located to the south-west of Gauteng province in north-east South Africa.</obo:IAO_0000115>
        <oboInOwl:hasOBONamespace>GAZ</oboInOwl:hasOBONamespace>
        <oboInOwl:id>GAZ:00076181</oboInOwl:id>
        <rdfs:label>Kromdraai Conservancy</rdfs:label>
    </owl:NamedIndividual>
    


    <!-- http://purl.obolibrary.org/obo/GAZ_00076182 -->

    <owl:NamedIndividual rdf:about="http://purl.obolibrary.org/obo/GAZ_00076182">
        <obo:RO_0001025 rdf:resource="http://purl.obolibrary.org/obo/GAZ_00009436"/>
        <obo:IAO_0000115>A 1 km2 reserve centered on a wild willowleaf fig tree Ficus salicifolia that is more than a thousand years old, found towards the north of the Magaliesberg Mountains in the Northern portion of the Tshwane (Pretoria) Metropole, South Africa.</obo:IAO_0000115>
        <oboInOwl:hasOBONamespace>GAZ</oboInOwl:hasOBONamespace>
        <oboInOwl:id>GAZ:00076182</oboInOwl:id>
        <rdfs:label>Wonderboom Nature Reserve</rdfs:label>
    </owl:NamedIndividual>
    


    <!-- http://purl.obolibrary.org/obo/GAZ_00076183 -->

    <owl:NamedIndividual rdf:about="http://purl.obolibrary.org/obo/GAZ_00076183">
        <obo:RO_0001025 rdf:resource="http://purl.obolibrary.org/obo/GAZ_00002815"/>
        <obo:IAO_0000115>A protected area in Gauteng Province.</obo:IAO_0000115>
        <oboInOwl:hasOBONamespace>GAZ</oboInOwl:hasOBONamespace>
        <oboInOwl:id>GAZ:00076183</oboInOwl:id>
        <rdfs:label>Abe Bailey Nature Reserve</rdfs:label>
    </owl:NamedIndividual>
    


    <!-- http://purl.obolibrary.org/obo/GAZ_00076184 -->

    <owl:NamedIndividual rdf:about="http://purl.obolibrary.org/obo/GAZ_00076184">
        <obo:RO_0001025 rdf:resource="http://purl.obolibrary.org/obo/GAZ_00002815"/>
        <obo:IAO_0000115>A protected area in Gauteng Province.</obo:IAO_0000115>
        <oboInOwl:hasOBONamespace>GAZ</oboInOwl:hasOBONamespace>
        <oboInOwl:id>GAZ:00076184</oboInOwl:id>
        <rdfs:label>Marievale Bird Sanctuary</rdfs:label>
    </owl:NamedIndividual>
    


    <!-- http://purl.obolibrary.org/obo/GAZ_00076185 -->

    <owl:NamedIndividual rdf:about="http://purl.obolibrary.org/obo/GAZ_00076185">
        <obo:RO_0001025 rdf:resource="http://purl.obolibrary.org/obo/GAZ_00002815"/>
        <obo:IAO_0000115>A protected area in Gauteng Province.</obo:IAO_0000115>
        <oboInOwl:hasOBONamespace>GAZ</oboInOwl:hasOBONamespace>
        <oboInOwl:id>GAZ:00076185</oboInOwl:id>
        <rdfs:label>Roodeplaat Nature Reserve</rdfs:label>
    </owl:NamedIndividual>
    


    <!-- http://purl.obolibrary.org/obo/GAZ_00076186 -->

    <owl:NamedIndividual rdf:about="http://purl.obolibrary.org/obo/GAZ_00076186">
        <obo:RO_0001025 rdf:resource="http://purl.obolibrary.org/obo/GAZ_00032879"/>
        <obo:IAO_0000115>A protected area near Johannesburg.</obo:IAO_0000115>
        <oboInOwl:hasOBONamespace>GAZ</oboInOwl:hasOBONamespace>
        <oboInOwl:id>GAZ:00076186</oboInOwl:id>
        <rdfs:label>Suikerbosrand Nature Reserve</rdfs:label>
    </owl:NamedIndividual>
    


    <!-- http://purl.obolibrary.org/obo/GAZ_00076187 -->

    <owl:NamedIndividual rdf:about="http://purl.obolibrary.org/obo/GAZ_00076187">
        <obo:RO_0001025 rdf:resource="http://purl.obolibrary.org/obo/GAZ_00002819"/>
        <obo:IAO_0000115>A protected area in Eastern Cape Province.</obo:IAO_0000115>
        <oboInOwl:hasOBONamespace>GAZ</oboInOwl:hasOBONamespace>
        <oboInOwl:id>GAZ:00076187</oboInOwl:id>
        <rdfs:label>Dwesa Provincial Park</rdfs:label>
    </owl:NamedIndividual>
    


    <!-- http://purl.obolibrary.org/obo/GAZ_00076188 -->

    <owl:NamedIndividual rdf:about="http://purl.obolibrary.org/obo/GAZ_00076188">
        <obo:RO_0001025 rdf:resource="http://purl.obolibrary.org/obo/GAZ_00076201"/>
        <obo:IAO_0000115>A protected area in Eastern Cape Province.</obo:IAO_0000115>
        <oboInOwl:hasOBONamespace>GAZ</oboInOwl:hasOBONamespace>
        <oboInOwl:id>GAZ:00076188</oboInOwl:id>
        <rdfs:label>Baviaanskloof Provincial Park</rdfs:label>
    </owl:NamedIndividual>
    


    <!-- http://purl.obolibrary.org/obo/GAZ_00076189 -->

    <owl:NamedIndividual rdf:about="http://purl.obolibrary.org/obo/GAZ_00076189">
        <obo:RO_0001025 rdf:resource="http://purl.obolibrary.org/obo/GAZ_00002819"/>
        <obo:IAO_0000115>A protected area in Eastern Cape Province.</obo:IAO_0000115>
        <oboInOwl:hasOBONamespace>GAZ</oboInOwl:hasOBONamespace>
        <oboInOwl:id>GAZ:00076189</oboInOwl:id>
        <rdfs:label>Tsolwana Provincial Park</rdfs:label>
    </owl:NamedIndividual>
    


    <!-- http://purl.obolibrary.org/obo/GAZ_00076190 -->

    <owl:NamedIndividual rdf:about="http://purl.obolibrary.org/obo/GAZ_00076190">
        <obo:RO_0001025 rdf:resource="http://purl.obolibrary.org/obo/GAZ_00002819"/>
        <obo:IAO_0000115>A protected area in Eastern Cape Province.</obo:IAO_0000115>
        <oboInOwl:hasOBONamespace>GAZ</oboInOwl:hasOBONamespace>
        <oboInOwl:id>GAZ:00076190</oboInOwl:id>
        <rdfs:label>Commando Drift Provincial Park</rdfs:label>
    </owl:NamedIndividual>
    


    <!-- http://purl.obolibrary.org/obo/GAZ_00076191 -->

    <owl:NamedIndividual rdf:about="http://purl.obolibrary.org/obo/GAZ_00076191">
        <obo:RO_0001025 rdf:resource="http://purl.obolibrary.org/obo/GAZ_00002819"/>
        <obo:IAO_0000115>A protected area in Eastern Cape Province.</obo:IAO_0000115>
        <oboInOwl:hasOBONamespace>GAZ</oboInOwl:hasOBONamespace>
        <oboInOwl:id>GAZ:00076191</oboInOwl:id>
        <rdfs:label>Great Fish River Provincial Park</rdfs:label>
    </owl:NamedIndividual>
    


    <!-- http://purl.obolibrary.org/obo/GAZ_00076192 -->

    <owl:NamedIndividual rdf:about="http://purl.obolibrary.org/obo/GAZ_00076192">
        <obo:RO_0001025 rdf:resource="http://purl.obolibrary.org/obo/GAZ_00002819"/>
        <obo:IAO_0000115>A protected area in Eastern Cape Province.</obo:IAO_0000115>
        <oboInOwl:hasOBONamespace>GAZ</oboInOwl:hasOBONamespace>
        <oboInOwl:id>GAZ:00076192</oboInOwl:id>
        <rdfs:label>Cwebe Provincial Park</rdfs:label>
    </owl:NamedIndividual>
    


    <!-- http://purl.obolibrary.org/obo/GAZ_00076193 -->

    <owl:NamedIndividual rdf:about="http://purl.obolibrary.org/obo/GAZ_00076193">
        <obo:RO_0001025 rdf:resource="http://purl.obolibrary.org/obo/GAZ_00002819"/>
        <obo:IAO_0000115>A protected area in Eastern Cape Province.</obo:IAO_0000115>
        <oboInOwl:hasOBONamespace>GAZ</oboInOwl:hasOBONamespace>
        <oboInOwl:id>GAZ:00076193</oboInOwl:id>
        <rdfs:label>East London Coast Provincial Park</rdfs:label>
    </owl:NamedIndividual>
    


    <!-- http://purl.obolibrary.org/obo/GAZ_00076194 -->

    <owl:NamedIndividual rdf:about="http://purl.obolibrary.org/obo/GAZ_00076194">
        <obo:RO_0001025 rdf:resource="http://purl.obolibrary.org/obo/GAZ_00002819"/>
        <obo:IAO_0000115>A protected area in Eastern Cape Province.</obo:IAO_0000115>
        <oboInOwl:hasOBONamespace>GAZ</oboInOwl:hasOBONamespace>
        <oboInOwl:id>GAZ:00076194</oboInOwl:id>
        <rdfs:label>Mkhambathi Provincial Park</rdfs:label>
    </owl:NamedIndividual>
    


    <!-- http://purl.obolibrary.org/obo/GAZ_00076195 -->

    <owl:NamedIndividual rdf:about="http://purl.obolibrary.org/obo/GAZ_00076195">
        <obo:RO_0001025 rdf:resource="http://purl.obolibrary.org/obo/GAZ_00002819"/>
        <obo:IAO_0000115>A protected area in Eastern Cape Province.</obo:IAO_0000115>
        <oboInOwl:hasOBONamespace>GAZ</oboInOwl:hasOBONamespace>
        <oboInOwl:id>GAZ:00076195</oboInOwl:id>
        <rdfs:label>Silaka Provincial Park</rdfs:label>
    </owl:NamedIndividual>
    


    <!-- http://purl.obolibrary.org/obo/GAZ_00076196 -->

    <owl:NamedIndividual rdf:about="http://purl.obolibrary.org/obo/GAZ_00076196">
        <obo:RO_0001025 rdf:resource="http://purl.obolibrary.org/obo/GAZ_00002819"/>
        <obo:IAO_0000115>A protected area in Eastern Cape Province.</obo:IAO_0000115>
        <oboInOwl:hasOBONamespace>GAZ</oboInOwl:hasOBONamespace>
        <oboInOwl:id>GAZ:00076196</oboInOwl:id>
        <rdfs:label>Fort Fordyce Provincial Park</rdfs:label>
    </owl:NamedIndividual>
    


    <!-- http://purl.obolibrary.org/obo/GAZ_00076197 -->

    <owl:NamedIndividual rdf:about="http://purl.obolibrary.org/obo/GAZ_00076197">
        <obo:RO_0001025 rdf:resource="http://purl.obolibrary.org/obo/GAZ_00002819"/>
        <obo:IAO_0000115>A protected area in Eastern Cape Province.</obo:IAO_0000115>
        <oboInOwl:hasOBONamespace>GAZ</oboInOwl:hasOBONamespace>
        <oboInOwl:id>GAZ:00076197</oboInOwl:id>
        <rdfs:label>Mpofu Provincial Park</rdfs:label>
    </owl:NamedIndividual>
    


    <!-- http://purl.obolibrary.org/obo/GAZ_00076199 -->

    <owl:NamedIndividual rdf:about="http://purl.obolibrary.org/obo/GAZ_00076199">
        <obo:RO_0001025 rdf:resource="http://purl.obolibrary.org/obo/GAZ_00002819"/>
        <obo:IAO_0000115>A protected area in Eastern Cape Province.</obo:IAO_0000115>
        <oboInOwl:hasOBONamespace>GAZ</oboInOwl:hasOBONamespace>
        <oboInOwl:id>GAZ:00076199</oboInOwl:id>
        <rdfs:label>Hluleka Provincial Park</rdfs:label>
    </owl:NamedIndividual>
    


    <!-- http://purl.obolibrary.org/obo/GAZ_00076200 -->

    <owl:NamedIndividual rdf:about="http://purl.obolibrary.org/obo/GAZ_00076200">
        <obo:RO_0001025 rdf:resource="http://purl.obolibrary.org/obo/GAZ_00002819"/>
        <obo:IAO_0000115>A protected area located approximately 30 km north-east of East London, and is situated within an area of 100 km2 encompassing five different biomes in the wild coast region of South Africa&apos;s Eastern Cape province.</obo:IAO_0000115>
        <oboInOwl:hasOBONamespace>GAZ</oboInOwl:hasOBONamespace>
        <oboInOwl:id>GAZ:00076200</oboInOwl:id>
        <rdfs:label>Inkwenkwezi Private Game Reserve</rdfs:label>
    </owl:NamedIndividual>
    


    <!-- http://purl.obolibrary.org/obo/GAZ_00076201 -->

    <owl:NamedIndividual rdf:about="http://purl.obolibrary.org/obo/GAZ_00076201">
        <obo:RO_0001025 rdf:resource="http://purl.obolibrary.org/obo/GAZ_00002819"/>
        <obo:IAO_0000115>A protected area in Eastern Cape Province. A World Heritage Site.</obo:IAO_0000115>
        <oboInOwl:hasOBONamespace>GAZ</oboInOwl:hasOBONamespace>
        <oboInOwl:id>GAZ:00076201</oboInOwl:id>
        <rdfs:label>Baviaanskloof Mega Reserve</rdfs:label>
    </owl:NamedIndividual>
    


    <!-- http://purl.obolibrary.org/obo/GAZ_00076202 -->

    <owl:NamedIndividual rdf:about="http://purl.obolibrary.org/obo/GAZ_00076202">
        <obo:RO_0001025 rdf:resource="http://purl.obolibrary.org/obo/GAZ_00002813"/>
        <obo:IAO_0000115>A protected area in Free State Province.</obo:IAO_0000115>
        <oboInOwl:hasOBONamespace>GAZ</oboInOwl:hasOBONamespace>
        <oboInOwl:id>GAZ:00076202</oboInOwl:id>
        <rdfs:label>Caledon Nature Reserve</rdfs:label>
    </owl:NamedIndividual>
    


    <!-- http://purl.obolibrary.org/obo/GAZ_00076203 -->

    <owl:NamedIndividual rdf:about="http://purl.obolibrary.org/obo/GAZ_00076203">
        <obo:RO_0001025 rdf:resource="http://purl.obolibrary.org/obo/GAZ_00002813"/>
        <obo:IAO_0000115>A protected area in Free State Province.</obo:IAO_0000115>
        <oboInOwl:hasOBONamespace>GAZ</oboInOwl:hasOBONamespace>
        <oboInOwl:id>GAZ:00076203</oboInOwl:id>
        <rdfs:label>Sandveld Nature Reserve</rdfs:label>
    </owl:NamedIndividual>
    


    <!-- http://purl.obolibrary.org/obo/GAZ_00076204 -->

    <owl:NamedIndividual rdf:about="http://purl.obolibrary.org/obo/GAZ_00076204">
        <obo:RO_0001025 rdf:resource="http://purl.obolibrary.org/obo/GAZ_00002813"/>
        <obo:IAO_0000115>A protected area in Free State Province.</obo:IAO_0000115>
        <oboInOwl:hasOBONamespace>GAZ</oboInOwl:hasOBONamespace>
        <oboInOwl:id>GAZ:00076204</oboInOwl:id>
        <rdfs:label>Soetdoring Nature Reserve</rdfs:label>
    </owl:NamedIndividual>
    


    <!-- http://purl.obolibrary.org/obo/GAZ_00076205 -->

    <owl:NamedIndividual rdf:about="http://purl.obolibrary.org/obo/GAZ_00076205">
        <obo:RO_0001025 rdf:resource="http://purl.obolibrary.org/obo/GAZ_00002813"/>
        <obo:IAO_0000115>A protected area in Free State Province.</obo:IAO_0000115>
        <oboInOwl:hasOBONamespace>GAZ</oboInOwl:hasOBONamespace>
        <oboInOwl:id>GAZ:00076205</oboInOwl:id>
        <rdfs:label>Tussen-die- Riviere Game Farm</rdfs:label>
    </owl:NamedIndividual>
    


    <!-- http://purl.obolibrary.org/obo/GAZ_00076206 -->

    <owl:NamedIndividual rdf:about="http://purl.obolibrary.org/obo/GAZ_00076206">
        <obo:RO_0001025 rdf:resource="http://purl.obolibrary.org/obo/GAZ_00002813"/>
        <obo:IAO_0000115>A protected area in Free State Province.</obo:IAO_0000115>
        <oboInOwl:hasOBONamespace>GAZ</oboInOwl:hasOBONamespace>
        <oboInOwl:id>GAZ:00076206</oboInOwl:id>
        <rdfs:label>Gariep Nature Reserve</rdfs:label>
    </owl:NamedIndividual>
    


    <!-- http://purl.obolibrary.org/obo/GAZ_00076207 -->

    <owl:NamedIndividual rdf:about="http://purl.obolibrary.org/obo/GAZ_00076207">
        <obo:RO_0001025 rdf:resource="http://purl.obolibrary.org/obo/GAZ_00002812"/>
        <obo:IAO_0000115>A game reserve in Maputaland, KwaZulu-Natal, South Africa. It is situated on the border with Mozambique where the Pongola River joins the Great Usutu River. It is adjacent to the Tembe Elephant Park.</obo:IAO_0000115>
        <oboInOwl:hasOBONamespace>GAZ</oboInOwl:hasOBONamespace>
        <oboInOwl:id>GAZ:00076207</oboInOwl:id>
        <rdfs:label>Ndumo Game Reserve</rdfs:label>
    </owl:NamedIndividual>
    


    <!-- http://purl.obolibrary.org/obo/GAZ_00076208 -->

    <owl:NamedIndividual rdf:about="http://purl.obolibrary.org/obo/GAZ_00076208">
        <obo:RO_0001025 rdf:resource="http://purl.obolibrary.org/obo/GAZ_00002812"/>
        <obo:IAO_0000115>A protected area in KwaZulu-Natal Province.</obo:IAO_0000115>
        <oboInOwl:hasOBONamespace>GAZ</oboInOwl:hasOBONamespace>
        <oboInOwl:id>GAZ:00076208</oboInOwl:id>
        <rdfs:label>Oribi Gorge Nature Reserve</rdfs:label>
    </owl:NamedIndividual>
    


    <!-- http://purl.obolibrary.org/obo/GAZ_00076209 -->

    <owl:NamedIndividual rdf:about="http://purl.obolibrary.org/obo/GAZ_00076209">
        <obo:RO_0001025 rdf:resource="http://purl.obolibrary.org/obo/GAZ_00002812"/>
        <obo:IAO_0000115>A protected area in KwaZulu-Natal Province.</obo:IAO_0000115>
        <oboInOwl:hasOBONamespace>GAZ</oboInOwl:hasOBONamespace>
        <oboInOwl:id>GAZ:00076209</oboInOwl:id>
        <rdfs:label>Umtamvuna Nature Reserve</rdfs:label>
    </owl:NamedIndividual>
    


    <!-- http://purl.obolibrary.org/obo/GAZ_00076210 -->

    <owl:NamedIndividual rdf:about="http://purl.obolibrary.org/obo/GAZ_00076210">
        <obo:RO_0001025 rdf:resource="http://purl.obolibrary.org/obo/GAZ_00002812"/>
        <obo:IAO_0000115>A protected area in KwaZulu-Natal Province.</obo:IAO_0000115>
        <oboInOwl:hasOBONamespace>GAZ</oboInOwl:hasOBONamespace>
        <oboInOwl:id>GAZ:00076210</oboInOwl:id>
        <rdfs:label>Spioenkop Dam Nature Reserve</rdfs:label>
    </owl:NamedIndividual>
    


    <!-- http://purl.obolibrary.org/obo/GAZ_00076211 -->

    <owl:NamedIndividual rdf:about="http://purl.obolibrary.org/obo/GAZ_00076211">
        <obo:RO_0001025 rdf:resource="http://purl.obolibrary.org/obo/GAZ_00002812"/>
        <obo:IAO_0000115>A protected area in KwaZulu-Natal Province.</obo:IAO_0000115>
        <oboInOwl:hasOBONamespace>GAZ</oboInOwl:hasOBONamespace>
        <oboInOwl:id>GAZ:00076211</oboInOwl:id>
        <rdfs:label>Midmar Nature Reserve</rdfs:label>
    </owl:NamedIndividual>
    


    <!-- http://purl.obolibrary.org/obo/GAZ_00076212 -->

    <owl:NamedIndividual rdf:about="http://purl.obolibrary.org/obo/GAZ_00076212">
        <obo:IAO_0000115>A series of interlinked lakes in the Maputuland area of KwaZulu-Natal, South Africa. The lakes form part of the Greater Saint Lucia Wetland Park, a World Heritage Site.</obo:IAO_0000115>
        <oboInOwl:hasOBONamespace>GAZ</oboInOwl:hasOBONamespace>
        <oboInOwl:id>GAZ:00076212</oboInOwl:id>
        <rdfs:label>Kosi Bay</rdfs:label>
    </owl:NamedIndividual>
    


    <!-- http://purl.obolibrary.org/obo/GAZ_00076214 -->

    <owl:NamedIndividual rdf:about="http://purl.obolibrary.org/obo/GAZ_00076214">
        <obo:RO_0001025 rdf:resource="http://purl.obolibrary.org/obo/GAZ_00005308"/>
        <oboInOwl:hasOBONamespace>GAZ</oboInOwl:hasOBONamespace>
        <oboInOwl:id>GAZ:00076214</oboInOwl:id>
        <rdfs:label>Lake Etrza Nature Reserve</rdfs:label>
    </owl:NamedIndividual>
    


    <!-- http://purl.obolibrary.org/obo/GAZ_00076215 -->

    <owl:NamedIndividual rdf:about="http://purl.obolibrary.org/obo/GAZ_00076215">
        <obo:RO_0001025 rdf:resource="http://purl.obolibrary.org/obo/GAZ_00005308"/>
        <obo:IAO_0000115>A protected area.</obo:IAO_0000115>
        <oboInOwl:hasOBONamespace>GAZ</oboInOwl:hasOBONamespace>
        <oboInOwl:id>GAZ:00076215</oboInOwl:id>
        <rdfs:label>Saint Lucia Marine Reserve</rdfs:label>
    </owl:NamedIndividual>
    


    <!-- http://purl.obolibrary.org/obo/GAZ_00076216 -->

    <owl:NamedIndividual rdf:about="http://purl.obolibrary.org/obo/GAZ_00076216">
        <obo:RO_0001025 rdf:resource="http://purl.obolibrary.org/obo/GAZ_00005308"/>
        <obo:IAO_0000115>A protected area. Located along the Western Shores of False Bay.</obo:IAO_0000115>
        <oboInOwl:hasOBONamespace>GAZ</oboInOwl:hasOBONamespace>
        <oboInOwl:id>GAZ:00076216</oboInOwl:id>
        <rdfs:label>False Bay Park</rdfs:label>
    </owl:NamedIndividual>
    


    <!-- http://purl.obolibrary.org/obo/GAZ_00076217 -->

    <owl:NamedIndividual rdf:about="http://purl.obolibrary.org/obo/GAZ_00076217">
        <obo:RO_0001025 rdf:resource="http://purl.obolibrary.org/obo/GAZ_00005308"/>
        <oboInOwl:hasOBONamespace>GAZ</oboInOwl:hasOBONamespace>
        <oboInOwl:id>GAZ:00076217</oboInOwl:id>
        <rdfs:label>Mapelane Nature Reserve</rdfs:label>
    </owl:NamedIndividual>
    


    <!-- http://purl.obolibrary.org/obo/GAZ_00076218 -->

    <owl:NamedIndividual rdf:about="http://purl.obolibrary.org/obo/GAZ_00076218">
        <obo:RO_0001025 rdf:resource="http://purl.obolibrary.org/obo/GAZ_00002812"/>
        <oboInOwl:hasOBONamespace>GAZ</oboInOwl:hasOBONamespace>
        <oboInOwl:id>GAZ:00076218</oboInOwl:id>
        <rdfs:label>Karkloof Nature Reserve</rdfs:label>
    </owl:NamedIndividual>
    


    <!-- http://purl.obolibrary.org/obo/GAZ_00076219 -->

    <owl:NamedIndividual rdf:about="http://purl.obolibrary.org/obo/GAZ_00076219">
        <obo:RO_0001025 rdf:resource="http://purl.obolibrary.org/obo/GAZ_00239785"/>
        <obo:IAO_0000115>A protected area. Located in the southern Drakensberg.</obo:IAO_0000115>
        <oboInOwl:hasOBONamespace>GAZ</oboInOwl:hasOBONamespace>
        <oboInOwl:id>GAZ:00076219</oboInOwl:id>
        <rdfs:label>Himeville Nature Reserve</rdfs:label>
    </owl:NamedIndividual>
    


    <!-- http://purl.obolibrary.org/obo/GAZ_00076220 -->

    <owl:NamedIndividual rdf:about="http://purl.obolibrary.org/obo/GAZ_00076220">
        <obo:RO_0001025 rdf:resource="http://purl.obolibrary.org/obo/GAZ_00002812"/>
        <obo:IAO_0000115>A protected area.</obo:IAO_0000115>
        <oboInOwl:hasOBONamespace>GAZ</oboInOwl:hasOBONamespace>
        <oboInOwl:id>GAZ:00076220</oboInOwl:id>
        <rdfs:label>Weenen Game Reserve</rdfs:label>
    </owl:NamedIndividual>
    


    <!-- http://purl.obolibrary.org/obo/GAZ_00076221 -->

    <owl:NamedIndividual rdf:about="http://purl.obolibrary.org/obo/GAZ_00076221">
        <obo:RO_0001025 rdf:resource="http://purl.obolibrary.org/obo/GAZ_00002812"/>
        <oboInOwl:hasOBONamespace>GAZ</oboInOwl:hasOBONamespace>
        <oboInOwl:id>GAZ:00076221</oboInOwl:id>
        <rdfs:label>Albert Falls Game Reserve</rdfs:label>
    </owl:NamedIndividual>
    


    <!-- http://purl.obolibrary.org/obo/GAZ_00076222 -->

    <owl:NamedIndividual rdf:about="http://purl.obolibrary.org/obo/GAZ_00076222">
        <obo:RO_0001025 rdf:resource="http://purl.obolibrary.org/obo/GAZ_00239719"/>
        <obo:IAO_0000115>A protected area. Located in Kloof, between Hillcrest and Pinetown, near Durban. Established 1950.</obo:IAO_0000115>
        <oboInOwl:hasOBONamespace>GAZ</oboInOwl:hasOBONamespace>
        <oboInOwl:id>GAZ:00076222</oboInOwl:id>
        <rdfs:label>Kranskloof Nature Reserve</rdfs:label>
    </owl:NamedIndividual>
    


    <!-- http://purl.obolibrary.org/obo/GAZ_00076223 -->

    <owl:NamedIndividual rdf:about="http://purl.obolibrary.org/obo/GAZ_00076223">
        <obo:RO_0001025 rdf:resource="http://purl.obolibrary.org/obo/GAZ_00075931"/>
        <oboInOwl:hasOBONamespace>GAZ</oboInOwl:hasOBONamespace>
        <oboInOwl:id>GAZ:00076223</oboInOwl:id>
        <rdfs:label>Pongolapoort Nature Reserve</rdfs:label>
    </owl:NamedIndividual>
    


    <!-- http://purl.obolibrary.org/obo/GAZ_00076224 -->

    <owl:NamedIndividual rdf:about="http://purl.obolibrary.org/obo/GAZ_00076224">
        <obo:RO_0001025 rdf:resource="http://purl.obolibrary.org/obo/GAZ_00075418"/>
        <obo:IAO_0000115>A national park that is part of the Waterberg Biosphere in Limpopo Province, South Africa.</obo:IAO_0000115>
        <oboInOwl:hasOBONamespace>GAZ</oboInOwl:hasOBONamespace>
        <oboInOwl:id>GAZ:00076224</oboInOwl:id>
        <rdfs:label>Marakele National Park</rdfs:label>
    </owl:NamedIndividual>
    


    <!-- http://purl.obolibrary.org/obo/GAZ_00076225 -->

    <owl:NamedIndividual rdf:about="http://purl.obolibrary.org/obo/GAZ_00076225">
        <obo:RO_0001025 rdf:resource="http://purl.obolibrary.org/obo/GAZ_00002812"/>
        <oboInOwl:hasOBONamespace>GAZ</oboInOwl:hasOBONamespace>
        <oboInOwl:id>GAZ:00076225</oboInOwl:id>
        <rdfs:label>Coleford Nature Reserve</rdfs:label>
    </owl:NamedIndividual>
    


    <!-- http://purl.obolibrary.org/obo/GAZ_00076226 -->

    <owl:NamedIndividual rdf:about="http://purl.obolibrary.org/obo/GAZ_00076226">
        <obo:RO_0001025 rdf:resource="http://purl.obolibrary.org/obo/GAZ_00002812"/>
        <oboInOwl:hasOBONamespace>GAZ</oboInOwl:hasOBONamespace>
        <oboInOwl:id>GAZ:00076226</oboInOwl:id>
        <rdfs:label>Richards Bay Game Reserve</rdfs:label>
    </owl:NamedIndividual>
    


    <!-- http://purl.obolibrary.org/obo/GAZ_00076227 -->

    <owl:NamedIndividual rdf:about="http://purl.obolibrary.org/obo/GAZ_00076227">
        <obo:RO_0001025 rdf:resource="http://purl.obolibrary.org/obo/GAZ_00002812"/>
        <obo:IAO_0000115>A coastal reserve situated 1 km from Mtunzini on the KwaZulu-Natal North Coast. Established 1948.</obo:IAO_0000115>
        <oboInOwl:hasOBONamespace>GAZ</oboInOwl:hasOBONamespace>
        <oboInOwl:id>GAZ:00076227</oboInOwl:id>
        <rdfs:label>Umlalazi Nature Reserve</rdfs:label>
    </owl:NamedIndividual>
    


    <!-- http://purl.obolibrary.org/obo/GAZ_00076228 -->

    <owl:NamedIndividual rdf:about="http://purl.obolibrary.org/obo/GAZ_00076228">
        <obo:RO_0001025 rdf:resource="http://purl.obolibrary.org/obo/GAZ_00002812"/>
        <obo:IAO_0000115>A protected area.</obo:IAO_0000115>
        <oboInOwl:hasOBONamespace>GAZ</oboInOwl:hasOBONamespace>
        <oboInOwl:id>GAZ:00076228</oboInOwl:id>
        <rdfs:label>Chelmsford Nature Reserve</rdfs:label>
    </owl:NamedIndividual>
    


    <!-- http://purl.obolibrary.org/obo/GAZ_00076229 -->

    <owl:NamedIndividual rdf:about="http://purl.obolibrary.org/obo/GAZ_00076229">
        <obo:RO_0001025 rdf:resource="http://purl.obolibrary.org/obo/GAZ_00239785"/>
        <obo:IAO_0000115>A protected area.</obo:IAO_0000115>
        <oboInOwl:hasOBONamespace>GAZ</oboInOwl:hasOBONamespace>
        <oboInOwl:id>GAZ:00076229</oboInOwl:id>
        <rdfs:label>Mount Currie Nature Reserve</rdfs:label>
    </owl:NamedIndividual>
    


    <!-- http://purl.obolibrary.org/obo/GAZ_00076230 -->

    <owl:NamedIndividual rdf:about="http://purl.obolibrary.org/obo/GAZ_00076230">
        <obo:RO_0001025 rdf:resource="http://purl.obolibrary.org/obo/GAZ_00002812"/>
        <oboInOwl:hasOBONamespace>GAZ</oboInOwl:hasOBONamespace>
        <oboInOwl:id>GAZ:00076230</oboInOwl:id>
        <rdfs:label>Shongweni Game Reserve</rdfs:label>
    </owl:NamedIndividual>
    


    <!-- http://purl.obolibrary.org/obo/GAZ_00076231 -->

    <owl:NamedIndividual rdf:about="http://purl.obolibrary.org/obo/GAZ_00076231">
        <obo:RO_0001025 rdf:resource="http://purl.obolibrary.org/obo/GAZ_00002812"/>
        <obo:IAO_0000115>A protected area.</obo:IAO_0000115>
        <oboInOwl:hasOBONamespace>GAZ</oboInOwl:hasOBONamespace>
        <oboInOwl:id>GAZ:00076231</oboInOwl:id>
        <rdfs:label>Vernon Crookes Nature Reserve</rdfs:label>
    </owl:NamedIndividual>
    


    <!-- http://purl.obolibrary.org/obo/GAZ_00076232 -->

    <owl:NamedIndividual rdf:about="http://purl.obolibrary.org/obo/GAZ_00076232">
        <obo:RO_0001025 rdf:resource="http://purl.obolibrary.org/obo/GAZ_00032882"/>
        <obo:IAO_0000115>A protected area in Limpopo Province. Established 1995.</obo:IAO_0000115>
        <oboInOwl:hasOBONamespace>GAZ</oboInOwl:hasOBONamespace>
        <oboInOwl:id>GAZ:00076232</oboInOwl:id>
        <rdfs:label>Mapungubwe National Park</rdfs:label>
    </owl:NamedIndividual>
    


    <!-- http://purl.obolibrary.org/obo/GAZ_00076234 -->

    <owl:NamedIndividual rdf:about="http://purl.obolibrary.org/obo/GAZ_00076234">
        <obo:RO_0001025 rdf:resource="http://purl.obolibrary.org/obo/GAZ_00002814"/>
        <obo:IAO_0000115>A protected area in Limpopo Province.</obo:IAO_0000115>
        <oboInOwl:hasOBONamespace>GAZ</oboInOwl:hasOBONamespace>
        <oboInOwl:id>GAZ:00076234</oboInOwl:id>
        <rdfs:label>Ben Alberts Nature Reserve</rdfs:label>
    </owl:NamedIndividual>
    


    <!-- http://purl.obolibrary.org/obo/GAZ_00076236 -->

    <owl:NamedIndividual rdf:about="http://purl.obolibrary.org/obo/GAZ_00076236">
        <obo:RO_0001025 rdf:resource="http://purl.obolibrary.org/obo/GAZ_00032881"/>
        <obo:IAO_0000115>A protected area in Limpopo Province.</obo:IAO_0000115>
        <oboInOwl:hasOBONamespace>GAZ</oboInOwl:hasOBONamespace>
        <oboInOwl:id>GAZ:00076236</oboInOwl:id>
        <rdfs:label>Mokolo Dam Nature Reserve</rdfs:label>
    </owl:NamedIndividual>
    


    <!-- http://purl.obolibrary.org/obo/GAZ_00076237 -->

    <owl:NamedIndividual rdf:about="http://purl.obolibrary.org/obo/GAZ_00076237">
        <obo:RO_0001025 rdf:resource="http://purl.obolibrary.org/obo/GAZ_00076238"/>
        <obo:IAO_0000115>A part of the Soutpansberg Mountain Range near Louis Trichardt, Limpopo Province, South Africa.</obo:IAO_0000115>
        <oboInOwl:hasOBONamespace>GAZ</oboInOwl:hasOBONamespace>
        <oboInOwl:id>GAZ:00076237</oboInOwl:id>
        <rdfs:label>Hanglip Reserve</rdfs:label>
    </owl:NamedIndividual>
    


    <!-- http://purl.obolibrary.org/obo/GAZ_00076238 -->

    <owl:NamedIndividual rdf:about="http://purl.obolibrary.org/obo/GAZ_00076238">
        <rdf:type rdf:resource="http://purl.obolibrary.org/obo/ENVO_00000106"/>
        <obo:RO_0001025 rdf:resource="http://purl.obolibrary.org/obo/GAZ_00002814"/>
        <obo:IAO_0000115>A range of mountains in the north of South Africa.</obo:IAO_0000115>
        <oboInOwl:hasOBONamespace>GAZ</oboInOwl:hasOBONamespace>
        <oboInOwl:id>GAZ:00076238</oboInOwl:id>
        <rdfs:label>Soutpansberg</rdfs:label>
    </owl:NamedIndividual>
    


    <!-- http://purl.obolibrary.org/obo/GAZ_00076239 -->

    <owl:NamedIndividual rdf:about="http://purl.obolibrary.org/obo/GAZ_00076239">
        <obo:RO_0001025 rdf:resource="http://purl.obolibrary.org/obo/GAZ_00032884"/>
        <obo:IAO_0000115>A mountain range.</obo:IAO_0000115>
        <oboInOwl:hasOBONamespace>GAZ</oboInOwl:hasOBONamespace>
        <oboInOwl:id>GAZ:00076239</oboInOwl:id>
        <rdfs:label>Blouberg</rdfs:label>
    </owl:NamedIndividual>
    


    <!-- http://purl.obolibrary.org/obo/GAZ_00076240 -->

    <owl:NamedIndividual rdf:about="http://purl.obolibrary.org/obo/GAZ_00076240">
        <obo:RO_0001025 rdf:resource="http://purl.obolibrary.org/obo/GAZ_00002809"/>
        <obo:IAO_0000115>An administrative region situated in the far North of the Kruger National Park, South Africa, and comprises approximately 240 km2 of land. The triangle is created by the confluence of the Limpopo and Luvuvhu rivers at Crook&apos;s Corner. The enclosed wedge of land touches on Mozambique at the confluence, and forms a border with Zimbabwe along the Limpopo River.</obo:IAO_0000115>
        <oboInOwl:hasOBONamespace>GAZ</oboInOwl:hasOBONamespace>
        <oboInOwl:id>GAZ:00076240</oboInOwl:id>
        <rdfs:label>Makuleke Region</rdfs:label>
    </owl:NamedIndividual>
    


    <!-- http://purl.obolibrary.org/obo/GAZ_00076241 -->

    <owl:NamedIndividual rdf:about="http://purl.obolibrary.org/obo/GAZ_00076241">
        <obo:RO_0001025 rdf:resource="http://purl.obolibrary.org/obo/GAZ_00076243"/>
        <obo:IAO_0000115>A game reserve located within the Sabi Sand Reserve, Mpumalanga province, South Africa.</obo:IAO_0000115>
        <oboInOwl:hasOBONamespace>GAZ</oboInOwl:hasOBONamespace>
        <oboInOwl:id>GAZ:00076241</oboInOwl:id>
        <rdfs:label>Mala Mala Reserve</rdfs:label>
    </owl:NamedIndividual>
    


    <!-- http://purl.obolibrary.org/obo/GAZ_00076242 -->

    <owl:NamedIndividual rdf:about="http://purl.obolibrary.org/obo/GAZ_00076242">
        <obo:RO_0001025 rdf:resource="http://purl.obolibrary.org/obo/GAZ_00002816"/>
        <obo:IAO_0000115>A protected area in Mpumalanga Province.</obo:IAO_0000115>
        <oboInOwl:hasOBONamespace>GAZ</oboInOwl:hasOBONamespace>
        <oboInOwl:id>GAZ:00076242</oboInOwl:id>
        <rdfs:label>Ohrigstad Dam Nature Reserve</rdfs:label>
    </owl:NamedIndividual>
    


    <!-- http://purl.obolibrary.org/obo/GAZ_00076243 -->

    <owl:NamedIndividual rdf:about="http://purl.obolibrary.org/obo/GAZ_00076243">
        <obo:RO_0001025 rdf:resource="http://purl.obolibrary.org/obo/GAZ_00002816"/>
        <obo:IAO_0000115>A private game reserve in South Africa, situated in the Sabi Sand Reserve which is in the South Western section of the Kruger National Park.</obo:IAO_0000115>
        <oboInOwl:hasOBONamespace>GAZ</oboInOwl:hasOBONamespace>
        <oboInOwl:id>GAZ:00076243</oboInOwl:id>
        <rdfs:label>Sabi-Sand Game Reserve</rdfs:label>
    </owl:NamedIndividual>
    


    <!-- http://purl.obolibrary.org/obo/GAZ_00076244 -->

    <owl:NamedIndividual rdf:about="http://purl.obolibrary.org/obo/GAZ_00076244">
        <obo:RO_0001025 rdf:resource="http://purl.obolibrary.org/obo/GAZ_00002816"/>
        <obo:IAO_0000115>A protected area in Mpumalanga Province.</obo:IAO_0000115>
        <oboInOwl:hasOBONamespace>GAZ</oboInOwl:hasOBONamespace>
        <oboInOwl:id>GAZ:00076244</oboInOwl:id>
        <rdfs:label>Josefsdal Songimvelo Game Reserve</rdfs:label>
    </owl:NamedIndividual>
    


    <!-- http://purl.obolibrary.org/obo/GAZ_00076245 -->

    <owl:NamedIndividual rdf:about="http://purl.obolibrary.org/obo/GAZ_00076245">
        <obo:RO_0001025 rdf:resource="http://purl.obolibrary.org/obo/GAZ_00002816"/>
        <obo:IAO_0000115>A protected area in Mpumalanga Province.</obo:IAO_0000115>
        <oboInOwl:hasOBONamespace>GAZ</oboInOwl:hasOBONamespace>
        <oboInOwl:id>GAZ:00076245</oboInOwl:id>
        <rdfs:label>SterkSpruit Nature Reserve</rdfs:label>
    </owl:NamedIndividual>
    


    <!-- http://purl.obolibrary.org/obo/GAZ_00076246 -->

    <owl:NamedIndividual rdf:about="http://purl.obolibrary.org/obo/GAZ_00076246">
        <obo:RO_0001025 rdf:resource="http://purl.obolibrary.org/obo/GAZ_00002816"/>
        <obo:IAO_0000115>A protected area in Mpumalanga Province.</obo:IAO_0000115>
        <oboInOwl:hasOBONamespace>GAZ</oboInOwl:hasOBONamespace>
        <oboInOwl:id>GAZ:00076246</oboInOwl:id>
        <rdfs:label>Loskop Dam Game Reserve</rdfs:label>
    </owl:NamedIndividual>
    


    <!-- http://purl.obolibrary.org/obo/GAZ_00076247 -->

    <owl:NamedIndividual rdf:about="http://purl.obolibrary.org/obo/GAZ_00076247">
        <obo:RO_0001025 rdf:resource="http://purl.obolibrary.org/obo/GAZ_00002816"/>
        <obo:IAO_0000115>A protected area in Mpumalanga Province.</obo:IAO_0000115>
        <oboInOwl:hasOBONamespace>GAZ</oboInOwl:hasOBONamespace>
        <oboInOwl:id>GAZ:00076247</oboInOwl:id>
        <rdfs:label>Nooitgedacht Dam Nature Reserve</rdfs:label>
    </owl:NamedIndividual>
    


    <!-- http://purl.obolibrary.org/obo/GAZ_00076248 -->

    <owl:NamedIndividual rdf:about="http://purl.obolibrary.org/obo/GAZ_00076248">
        <obo:RO_0001025 rdf:resource="http://purl.obolibrary.org/obo/GAZ_00002816"/>
        <obo:IAO_0000115>A protected area in Mpumalanga Province.</obo:IAO_0000115>
        <oboInOwl:hasOBONamespace>GAZ</oboInOwl:hasOBONamespace>
        <oboInOwl:id>GAZ:00076248</oboInOwl:id>
        <rdfs:label>Mthethomusha Game Reserve</rdfs:label>
    </owl:NamedIndividual>
    


    <!-- http://purl.obolibrary.org/obo/GAZ_00076249 -->

    <owl:NamedIndividual rdf:about="http://purl.obolibrary.org/obo/GAZ_00076249">
        <obo:RO_0001025 rdf:resource="http://purl.obolibrary.org/obo/GAZ_00239907"/>
        <obo:IAO_0000115>A significant natural feature of South Africa, located in Mpumalanga, and forming the northern part of the Drakensberg escarpment. It is 26 km in length and about 800 meters deep, mostly consisting of red sandstone. It is the third largest canyon in the world.</obo:IAO_0000115>
        <oboInOwl:hasOBONamespace>GAZ</oboInOwl:hasOBONamespace>
        <oboInOwl:id>GAZ:00076249</oboInOwl:id>
        <rdfs:label>Blyde River Canyon</rdfs:label>
    </owl:NamedIndividual>
    


    <!-- http://purl.obolibrary.org/obo/GAZ_00076250 -->

    <owl:NamedIndividual rdf:about="http://purl.obolibrary.org/obo/GAZ_00076250">
        <obo:RO_0001025 rdf:resource="http://purl.obolibrary.org/obo/GAZ_00076243"/>
        <obo:IAO_0000115>A protected area in Mpumalanga Province.</obo:IAO_0000115>
        <oboInOwl:hasOBONamespace>GAZ</oboInOwl:hasOBONamespace>
        <oboInOwl:id>GAZ:00076250</oboInOwl:id>
        <rdfs:label>Londolozi Game Reserve</rdfs:label>
    </owl:NamedIndividual>
    


    <!-- http://purl.obolibrary.org/obo/GAZ_00076251 -->

    <owl:NamedIndividual rdf:about="http://purl.obolibrary.org/obo/GAZ_00076251">
        <obo:RO_0001025 rdf:resource="http://purl.obolibrary.org/obo/GAZ_00002818"/>
        <obo:IAO_0000115>A national park in Northern Cape Province. Established 1999-08.</obo:IAO_0000115>
        <oboInOwl:hasOBONamespace>GAZ</oboInOwl:hasOBONamespace>
        <oboInOwl:id>GAZ:00076251</oboInOwl:id>
        <rdfs:label>Namaqua National Park</rdfs:label>
    </owl:NamedIndividual>
    


    <!-- http://purl.obolibrary.org/obo/GAZ_00076252 -->

    <owl:NamedIndividual rdf:about="http://purl.obolibrary.org/obo/GAZ_00076252">
        <obo:RO_0001025 rdf:resource="http://purl.obolibrary.org/obo/GAZ_00057762"/>
        <oboInOwl:hasOBONamespace>GAZ</oboInOwl:hasOBONamespace>
        <oboInOwl:id>GAZ:00076252</oboInOwl:id>
        <rdfs:label>Richtersveld National Park</rdfs:label>
    </owl:NamedIndividual>
    


    <!-- http://purl.obolibrary.org/obo/GAZ_00076253 -->

    <owl:NamedIndividual rdf:about="http://purl.obolibrary.org/obo/GAZ_00076253">
        <obo:RO_0001025 rdf:resource="http://purl.obolibrary.org/obo/GAZ_00002818"/>
        <obo:RO_0001025 rdf:resource="http://purl.obolibrary.org/obo/GAZ_00076157"/>
        <obo:IAO_0000115>A Scientific National Park in South Africa. The park lies about 70 km due west of Sutherland, South Africa near the border of the Northern Cape and Western Cape, in one of the most arid regions of South Africa, receiving 50 to 70 Municipality of precipitation in an average year.</obo:IAO_0000115>
        <oboInOwl:hasOBONamespace>GAZ</oboInOwl:hasOBONamespace>
        <oboInOwl:id>GAZ:00076253</oboInOwl:id>
        <rdfs:label>Tankwa Karoo National Park</rdfs:label>
    </owl:NamedIndividual>
    


    <!-- http://purl.obolibrary.org/obo/GAZ_00076254 -->

    <owl:NamedIndividual rdf:about="http://purl.obolibrary.org/obo/GAZ_00076254">
        <obo:RO_0001025 rdf:resource="http://purl.obolibrary.org/obo/GAZ_00002818"/>
        <obo:IAO_0000115>A national park located about 120 km west of Upington in the Northern Cape Province, South Africa. The Augrabies Falls National Park covers an area of 820 km2 and stretches along the Orange River. Established 1966.</obo:IAO_0000115>
        <oboInOwl:hasOBONamespace>GAZ</oboInOwl:hasOBONamespace>
        <oboInOwl:id>GAZ:00076254</oboInOwl:id>
        <rdfs:label>Augrabies Falls National Park</rdfs:label>
    </owl:NamedIndividual>
    


    <!-- http://purl.obolibrary.org/obo/GAZ_00076255 -->

    <owl:NamedIndividual rdf:about="http://purl.obolibrary.org/obo/GAZ_00076255">
        <obo:RO_0001025 rdf:resource="http://purl.obolibrary.org/obo/GAZ_00002818"/>
        <obo:IAO_0000115>A national park in Northern Cape Province.</obo:IAO_0000115>
        <oboInOwl:hasOBONamespace>GAZ</oboInOwl:hasOBONamespace>
        <oboInOwl:id>GAZ:00076255</oboInOwl:id>
        <rdfs:label>Vaalbos National Park</rdfs:label>
    </owl:NamedIndividual>
    


    <!-- http://purl.obolibrary.org/obo/GAZ_00076256 -->

    <owl:NamedIndividual rdf:about="http://purl.obolibrary.org/obo/GAZ_00076256">
        <obo:RO_0001025 rdf:resource="http://purl.obolibrary.org/obo/GAZ_00002818"/>
        <obo:IAO_0000115>A national park in Northern Cape Province.</obo:IAO_0000115>
        <oboInOwl:hasOBONamespace>GAZ</oboInOwl:hasOBONamespace>
        <oboInOwl:id>GAZ:00076256</oboInOwl:id>
        <rdfs:label>Goegab Nature Reserve</rdfs:label>
    </owl:NamedIndividual>
    


    <!-- http://purl.obolibrary.org/obo/GAZ_00076257 -->

    <owl:NamedIndividual rdf:about="http://purl.obolibrary.org/obo/GAZ_00076257">
        <obo:RO_0001025 rdf:resource="http://purl.obolibrary.org/obo/GAZ_00002818"/>
        <obo:IAO_0000115>A national park in Northern Cape Province.</obo:IAO_0000115>
        <oboInOwl:hasOBONamespace>GAZ</oboInOwl:hasOBONamespace>
        <oboInOwl:id>GAZ:00076257</oboInOwl:id>
        <rdfs:label>Spitskop Nature Reserve</rdfs:label>
    </owl:NamedIndividual>
    


    <!-- http://purl.obolibrary.org/obo/GAZ_00076258 -->

    <owl:NamedIndividual rdf:about="http://purl.obolibrary.org/obo/GAZ_00076258">
        <obo:RO_0001025 rdf:resource="http://purl.obolibrary.org/obo/GAZ_00002811"/>
        <obo:IAO_0000115>A national park in North West Province.</obo:IAO_0000115>
        <oboInOwl:hasOBONamespace>GAZ</oboInOwl:hasOBONamespace>
        <oboInOwl:id>GAZ:00076258</oboInOwl:id>
        <rdfs:label>Borakalalo National Park</rdfs:label>
    </owl:NamedIndividual>
    


    <!-- http://purl.obolibrary.org/obo/GAZ_00076259 -->

    <owl:NamedIndividual rdf:about="http://purl.obolibrary.org/obo/GAZ_00076259">
        <obo:RO_0001025 rdf:resource="http://purl.obolibrary.org/obo/GAZ_00032877"/>
        <obo:IAO_0000115>A national park that is located in North West Province in South Africa, west of Pretoria. The park borders with the entertainment complex Sun City. Also a District Management Area.</obo:IAO_0000115>
        <oboInOwl:hasOBONamespace>GAZ</oboInOwl:hasOBONamespace>
        <oboInOwl:id>GAZ:00076259</oboInOwl:id>
        <rdfs:label>Pilanesberg National Park</rdfs:label>
    </owl:NamedIndividual>
    


    <!-- http://purl.obolibrary.org/obo/GAZ_00076260 -->

    <owl:NamedIndividual rdf:about="http://purl.obolibrary.org/obo/GAZ_00076260">
        <obo:RO_0001025 rdf:resource="http://purl.obolibrary.org/obo/GAZ_00032875"/>
        <obo:IAO_0000115>A protected area in North West Province.</obo:IAO_0000115>
        <oboInOwl:hasOBONamespace>GAZ</oboInOwl:hasOBONamespace>
        <oboInOwl:id>GAZ:00076260</oboInOwl:id>
        <rdfs:label>Bloemhof Dam Nature Reserve</rdfs:label>
    </owl:NamedIndividual>
    


    <!-- http://purl.obolibrary.org/obo/GAZ_00076262 -->

    <owl:NamedIndividual rdf:about="http://purl.obolibrary.org/obo/GAZ_00076262">
        <obo:RO_0001025 rdf:resource="http://purl.obolibrary.org/obo/GAZ_00032877"/>
        <obo:IAO_0000115>A protected area in North West Province.</obo:IAO_0000115>
        <oboInOwl:hasOBONamespace>GAZ</oboInOwl:hasOBONamespace>
        <oboInOwl:id>GAZ:00076262</oboInOwl:id>
        <rdfs:label>Marico Bosveld Nature Reserve</rdfs:label>
    </owl:NamedIndividual>
    


    <!-- http://purl.obolibrary.org/obo/GAZ_00076263 -->

    <owl:NamedIndividual rdf:about="http://purl.obolibrary.org/obo/GAZ_00076263">
        <obo:RO_0001025 rdf:resource="http://purl.obolibrary.org/obo/GAZ_00032875"/>
        <obo:IAO_0000115>A protected area in North West Province.</obo:IAO_0000115>
        <oboInOwl:hasOBONamespace>GAZ</oboInOwl:hasOBONamespace>
        <oboInOwl:id>GAZ:00076263</oboInOwl:id>
        <rdfs:label>S.A. Lombard Nature Reserve</rdfs:label>
    </owl:NamedIndividual>
    


    <!-- http://purl.obolibrary.org/obo/GAZ_00076264 -->

    <owl:NamedIndividual rdf:about="http://purl.obolibrary.org/obo/GAZ_00076264">
        <obo:RO_0001025 rdf:resource="http://purl.obolibrary.org/obo/GAZ_00002811"/>
        <obo:IAO_0000115>A protected area in North West Province.</obo:IAO_0000115>
        <oboInOwl:hasOBONamespace>GAZ</oboInOwl:hasOBONamespace>
        <oboInOwl:id>GAZ:00076264</oboInOwl:id>
        <rdfs:label>Magaliesberg Natural Area</rdfs:label>
    </owl:NamedIndividual>
    


    <!-- http://purl.obolibrary.org/obo/GAZ_00076266 -->

    <owl:NamedIndividual rdf:about="http://purl.obolibrary.org/obo/GAZ_00076266">
        <obo:RO_0001025 rdf:resource="http://purl.obolibrary.org/obo/GAZ_00032876"/>
        <obo:IAO_0000115>A protected area in North West Province.</obo:IAO_0000115>
        <oboInOwl:hasOBONamespace>GAZ</oboInOwl:hasOBONamespace>
        <oboInOwl:id>GAZ:00076266</oboInOwl:id>
        <rdfs:label>Molopo Nature Reserve</rdfs:label>
    </owl:NamedIndividual>
    


    <!-- http://purl.obolibrary.org/obo/GAZ_00076267 -->

    <owl:NamedIndividual rdf:about="http://purl.obolibrary.org/obo/GAZ_00076267">
        <obo:RO_0001025 rdf:resource="http://purl.obolibrary.org/obo/GAZ_00032856"/>
        <obo:IAO_0000115>A national park in Western Cape Province.</obo:IAO_0000115>
        <oboInOwl:hasOBONamespace>GAZ</oboInOwl:hasOBONamespace>
        <oboInOwl:id>GAZ:00076267</oboInOwl:id>
        <rdfs:label>West Coast National Park</rdfs:label>
    </owl:NamedIndividual>
    


    <!-- http://purl.obolibrary.org/obo/GAZ_00076269 -->

    <owl:NamedIndividual rdf:about="http://purl.obolibrary.org/obo/GAZ_00076269">
        <obo:RO_0001025 rdf:resource="http://purl.obolibrary.org/obo/GAZ_00032845"/>
        <obo:IAO_0000115>A national park in Western Cape Province.</obo:IAO_0000115>
        <oboInOwl:hasOBONamespace>GAZ</oboInOwl:hasOBONamespace>
        <oboInOwl:id>GAZ:00076269</oboInOwl:id>
        <rdfs:label>Agulhas National Park</rdfs:label>
    </owl:NamedIndividual>
    


    <!-- http://purl.obolibrary.org/obo/GAZ_00076270 -->

    <owl:NamedIndividual rdf:about="http://purl.obolibrary.org/obo/GAZ_00076270">
        <obo:RO_0001025 rdf:resource="http://purl.obolibrary.org/obo/GAZ_00032845"/>
        <obo:IAO_0000115>A nature reserve in the Western Cape Province of South Africa. Located in Overberg region, near Agulhas, the southern tip of Africa. Established 1957.</obo:IAO_0000115>
        <oboInOwl:hasOBONamespace>GAZ</oboInOwl:hasOBONamespace>
        <oboInOwl:id>GAZ:00076270</oboInOwl:id>
        <rdfs:label>De Hoop Nature Reserve</rdfs:label>
    </owl:NamedIndividual>
    


    <!-- http://purl.obolibrary.org/obo/GAZ_00076271 -->

    <owl:NamedIndividual rdf:about="http://purl.obolibrary.org/obo/GAZ_00076271">
        <obo:RO_0001025 rdf:resource="http://purl.obolibrary.org/obo/GAZ_00032845"/>
        <obo:IAO_0000115>A national park in South Africa. It is the smallest of South Africa&apos;s national parks, covering an area of 27.86 km2. The park is part of the Cape Floral System, which is a World Heritage Site. The park is located 6 km south of Swellendam, in the foothills of the Langeberg Mountains. It is bordered to the south by the Breede River. Established 1961.</obo:IAO_0000115>
        <oboInOwl:hasOBONamespace>GAZ</oboInOwl:hasOBONamespace>
        <oboInOwl:id>GAZ:00076271</oboInOwl:id>
        <rdfs:label>Bontebok National Park</rdfs:label>
    </owl:NamedIndividual>
    


    <!-- http://purl.obolibrary.org/obo/GAZ_00076272 -->

    <owl:NamedIndividual rdf:about="http://purl.obolibrary.org/obo/GAZ_00076272">
        <obo:RO_0001025 rdf:resource="http://purl.obolibrary.org/obo/GAZ_00032855"/>
        <obo:RO_0001025 rdf:resource="http://purl.obolibrary.org/obo/GAZ_00076157"/>
        <obo:IAO_0000115>A national park in the isolated Karoo area of the Western Cape, South Africa near Beaufort West. Established 1979.</obo:IAO_0000115>
        <oboInOwl:hasOBONamespace>GAZ</oboInOwl:hasOBONamespace>
        <oboInOwl:id>GAZ:00076272</oboInOwl:id>
        <rdfs:label>Karoo National Park</rdfs:label>
    </owl:NamedIndividual>
    


    <!-- http://purl.obolibrary.org/obo/GAZ_00076274 -->

    <owl:NamedIndividual rdf:about="http://purl.obolibrary.org/obo/GAZ_00076274">
        <obo:RO_0001025 rdf:resource="http://purl.obolibrary.org/obo/GAZ_00032845"/>
        <obo:RO_0001025 rdf:resource="http://purl.obolibrary.org/obo/GAZ_00076151"/>
        <obo:IAO_0000115>A protected area situated 20 km north of Heidelberg in the Langeberg Mountains of the Western Cape Province, South Africa.</obo:IAO_0000115>
        <oboInOwl:hasOBONamespace>GAZ</oboInOwl:hasOBONamespace>
        <oboInOwl:id>GAZ:00076274</oboInOwl:id>
        <rdfs:label>Boosmansbos Wilderness Area</rdfs:label>
    </owl:NamedIndividual>
    


    <!-- http://purl.obolibrary.org/obo/GAZ_00076275 -->

    <owl:NamedIndividual rdf:about="http://purl.obolibrary.org/obo/GAZ_00076275">
        <obo:RO_0001025 rdf:resource="http://purl.obolibrary.org/obo/GAZ_00009437"/>
        <obo:IAO_0000115>A national park in Cape Town, South Africa, proclaimed on 1998-05029 for the purpose of protecting the natural environment of the Table Mountain Chain, and in particular the rare fynbos vegetation.</obo:IAO_0000115>
        <oboInOwl:hasOBONamespace>GAZ</oboInOwl:hasOBONamespace>
        <oboInOwl:id>GAZ:00076275</oboInOwl:id>
        <rdfs:label>Table Mountain National Park</rdfs:label>
    </owl:NamedIndividual>
    


    <!-- http://purl.obolibrary.org/obo/GAZ_00076276 -->

    <owl:NamedIndividual rdf:about="http://purl.obolibrary.org/obo/GAZ_00076276">
        <obo:RO_0001025 rdf:resource="http://purl.obolibrary.org/obo/GAZ_00012790"/>
        <obo:RO_0001025 rdf:resource="http://purl.obolibrary.org/obo/GAZ_00076136"/>
        <obo:IAO_0000115>A protected area in Western Cape Province.</obo:IAO_0000115>
        <oboInOwl:hasOBONamespace>GAZ</oboInOwl:hasOBONamespace>
        <oboInOwl:id>GAZ:00076276</oboInOwl:id>
        <rdfs:label>Hottentots-Holland Nature Reserve</rdfs:label>
    </owl:NamedIndividual>
    


    <!-- http://purl.obolibrary.org/obo/GAZ_00076277 -->

    <owl:NamedIndividual rdf:about="http://purl.obolibrary.org/obo/GAZ_00076277">
        <obo:RO_0001025 rdf:resource="http://purl.obolibrary.org/obo/GAZ_00076120"/>
        <obo:IAO_0000115>A protected area in Western Cape Province. Located in the Little Karoo, lying between the Swartberg and Outeniqua mountains.</obo:IAO_0000115>
        <oboInOwl:hasOBONamespace>GAZ</oboInOwl:hasOBONamespace>
        <oboInOwl:id>GAZ:00076277</oboInOwl:id>
        <rdfs:label>Gamka Mountain Nature Reserve</rdfs:label>
    </owl:NamedIndividual>
    


    <!-- http://purl.obolibrary.org/obo/GAZ_00076278 -->

    <owl:NamedIndividual rdf:about="http://purl.obolibrary.org/obo/GAZ_00076278">
        <obo:RO_0001025 rdf:resource="http://purl.obolibrary.org/obo/GAZ_00076120"/>
        <obo:IAO_0000115>A protected area in Western Cape Province. Located the Oudtshoorn district between the Great and Klein Karoo. It is bordered by the Gamkapoort Nature Reserve immediately to the north and Towerkop Nature Reserve immediately to the west.</obo:IAO_0000115>
        <oboInOwl:hasOBONamespace>GAZ</oboInOwl:hasOBONamespace>
        <oboInOwl:id>GAZ:00076278</oboInOwl:id>
        <rdfs:label>Swartberg Nature Reserve</rdfs:label>
    </owl:NamedIndividual>
    


    <!-- http://purl.obolibrary.org/obo/GAZ_00076279 -->

    <owl:NamedIndividual rdf:about="http://purl.obolibrary.org/obo/GAZ_00076279">
        <obo:RO_0001025 rdf:resource="http://purl.obolibrary.org/obo/GAZ_00076125"/>
        <obo:RO_0001025 rdf:resource="http://purl.obolibrary.org/obo/GAZ_00076151"/>
        <obo:IAO_0000115>A protected area that lies in the Swellendam mountains, between the towns of Swellendam, Ashton, Barrydale and Suurbraak.</obo:IAO_0000115>
        <oboInOwl:hasOBONamespace>GAZ</oboInOwl:hasOBONamespace>
        <oboInOwl:id>GAZ:00076279</oboInOwl:id>
        <rdfs:label>Marloth Nature Reserve</rdfs:label>
    </owl:NamedIndividual>
    


    <!-- http://purl.obolibrary.org/obo/GAZ_00076280 -->

    <owl:NamedIndividual rdf:about="http://purl.obolibrary.org/obo/GAZ_00076280">
        <obo:RO_0001025 rdf:resource="http://purl.obolibrary.org/obo/GAZ_00012790"/>
        <obo:IAO_0000115>A protected area in Western Cape Province. Located in the Breede River valley.</obo:IAO_0000115>
        <oboInOwl:hasOBONamespace>GAZ</oboInOwl:hasOBONamespace>
        <oboInOwl:id>GAZ:00076280</oboInOwl:id>
        <rdfs:label>Vrolijkheid Nature Reserve</rdfs:label>
    </owl:NamedIndividual>
    


    <!-- http://purl.obolibrary.org/obo/GAZ_00076281 -->

    <owl:NamedIndividual rdf:about="http://purl.obolibrary.org/obo/GAZ_00076281">
        <obo:RO_0001025 rdf:resource="http://purl.obolibrary.org/obo/GAZ_00032845"/>
        <obo:IAO_0000115>A protected area in Western Cape Province. Located 20 km east of Stanford, at the foot of the Perdeberg mountains. Established 1962.</obo:IAO_0000115>
        <oboInOwl:hasOBONamespace>GAZ</oboInOwl:hasOBONamespace>
        <oboInOwl:id>GAZ:00076281</oboInOwl:id>
        <rdfs:label>Salmons Dam Nature Reserve</rdfs:label>
    </owl:NamedIndividual>
    


    <!-- http://purl.obolibrary.org/obo/GAZ_00076282 -->

    <owl:NamedIndividual rdf:about="http://purl.obolibrary.org/obo/GAZ_00076282">
        <obo:RO_0001025 rdf:resource="http://purl.obolibrary.org/obo/GAZ_00076275"/>
        <obo:IAO_0000115>A flat-topped mountain forming a prominent landmark overlooking the city of Cape Town in South Africa.</obo:IAO_0000115>
        <oboInOwl:hasOBONamespace>GAZ</oboInOwl:hasOBONamespace>
        <oboInOwl:id>GAZ:00076282</oboInOwl:id>
        <rdfs:label>Table Mountain</rdfs:label>
    </owl:NamedIndividual>
    


    <!-- http://purl.obolibrary.org/obo/GAZ_00076283 -->

    <owl:NamedIndividual rdf:about="http://purl.obolibrary.org/obo/GAZ_00076283">
        <obo:RO_0001025 rdf:resource="http://purl.obolibrary.org/obo/GAZ_00076275"/>
        <obo:IAO_0000115>A botanical garden nestled at the foot of Table Mountain in Cape Town.</obo:IAO_0000115>
        <oboInOwl:hasOBONamespace>GAZ</oboInOwl:hasOBONamespace>
        <oboInOwl:id>GAZ:00076283</oboInOwl:id>
        <rdfs:label>Kirstenbosch National Botanical Garden</rdfs:label>
    </owl:NamedIndividual>
    


    <!-- http://purl.obolibrary.org/obo/GAZ_00076291 -->

    <owl:NamedIndividual rdf:about="http://purl.obolibrary.org/obo/GAZ_00076291">
        <obo:RO_0001025 rdf:resource="http://purl.obolibrary.org/obo/GAZ_00075422"/>
        <obo:IAO_0000115>A national park in Botswana.</obo:IAO_0000115>
        <oboInOwl:hasOBONamespace>GAZ</oboInOwl:hasOBONamespace>
        <oboInOwl:id>GAZ:00076291</oboInOwl:id>
        <rdfs:label>Nxai Pan National Park</rdfs:label>
    </owl:NamedIndividual>
    


    <!-- http://purl.obolibrary.org/obo/GAZ_00076293 -->

    <owl:NamedIndividual rdf:about="http://purl.obolibrary.org/obo/GAZ_00076293">
        <obo:IAO_0000115>A national park in Botswana. Established 1971.</obo:IAO_0000115>
        <oboInOwl:hasOBONamespace>GAZ</oboInOwl:hasOBONamespace>
        <oboInOwl:id>GAZ:00076293</oboInOwl:id>
        <rdfs:label>Khutse Game Reserve</rdfs:label>
    </owl:NamedIndividual>
    


    <!-- http://purl.obolibrary.org/obo/GAZ_00076641 -->

    <owl:NamedIndividual rdf:about="http://purl.obolibrary.org/obo/GAZ_00076641">
        <obo:IAO_0000115>One of the largest canyons in the world (definitely the largest in Africa). It features a gigantic ravine, in total about 160 km long, up to 27 km wide and in places almost 550 m deep.</obo:IAO_0000115>
        <oboInOwl:hasOBONamespace>GAZ</oboInOwl:hasOBONamespace>
        <oboInOwl:id>GAZ:00076641</oboInOwl:id>
        <rdfs:label>Fish River Canyon</rdfs:label>
    </owl:NamedIndividual>
    


    <!-- http://purl.obolibrary.org/obo/GAZ_00076643 -->

    <owl:NamedIndividual rdf:about="http://purl.obolibrary.org/obo/GAZ_00076643">
        <obo:IAO_0000115>An isolated Nature Reserve situated in the Kalahari Desert at the &apos;root&apos; of the Caprivi Strip in northeast of Namibia.</obo:IAO_0000115>
        <oboInOwl:hasOBONamespace>GAZ</oboInOwl:hasOBONamespace>
        <oboInOwl:id>GAZ:00076643</oboInOwl:id>
        <rdfs:label>Khaudom National Park</rdfs:label>
    </owl:NamedIndividual>
    


    <!-- http://purl.obolibrary.org/obo/GAZ_00076696 -->

    <owl:NamedIndividual rdf:about="http://purl.obolibrary.org/obo/GAZ_00076696">
        <obo:IAO_0000115>A national park in Swaziland.</obo:IAO_0000115>
        <oboInOwl:hasOBONamespace>GAZ</oboInOwl:hasOBONamespace>
        <oboInOwl:id>GAZ:00076696</oboInOwl:id>
        <rdfs:label>Mlawula National Park</rdfs:label>
    </owl:NamedIndividual>
    


    <!-- http://purl.obolibrary.org/obo/GAZ_00076762 -->

    <owl:NamedIndividual rdf:about="http://purl.obolibrary.org/obo/GAZ_00076762">
        <obo:IAO_0000115>A protected area in south-western Zimbabwe. It comprises four areas within the Zimbabwe national parks system and covers the entire west bank of the Shashe River within the Thuli Circle.</obo:IAO_0000115>
        <oboInOwl:hasOBONamespace>GAZ</oboInOwl:hasOBONamespace>
        <oboInOwl:id>GAZ:00076762</oboInOwl:id>
        <rdfs:label>Thuli Parks and Wildlife Land</rdfs:label>
    </owl:NamedIndividual>
    


    <!-- http://purl.obolibrary.org/obo/GAZ_00076763 -->

    <owl:NamedIndividual rdf:about="http://purl.obolibrary.org/obo/GAZ_00076763">
        <obo:RO_0001025 rdf:resource="http://purl.obolibrary.org/obo/GAZ_00076762"/>
        <oboInOwl:hasOBONamespace>GAZ</oboInOwl:hasOBONamespace>
        <oboInOwl:id>GAZ:00076763</oboInOwl:id>
        <rdfs:label>South Camp Botanical Reserve</rdfs:label>
    </owl:NamedIndividual>
    


    <!-- http://purl.obolibrary.org/obo/GAZ_00076764 -->

    <owl:NamedIndividual rdf:about="http://purl.obolibrary.org/obo/GAZ_00076764">
        <obo:RO_0001025 rdf:resource="http://purl.obolibrary.org/obo/GAZ_00076762"/>
        <oboInOwl:hasOBONamespace>GAZ</oboInOwl:hasOBONamespace>
        <oboInOwl:id>GAZ:00076764</oboInOwl:id>
        <rdfs:label>Pioneer Botanical Reserve</rdfs:label>
    </owl:NamedIndividual>
    


    <!-- http://purl.obolibrary.org/obo/GAZ_00076765 -->

    <owl:NamedIndividual rdf:about="http://purl.obolibrary.org/obo/GAZ_00076765">
        <obo:RO_0001025 rdf:resource="http://purl.obolibrary.org/obo/GAZ_00076762"/>
        <oboInOwl:hasOBONamespace>GAZ</oboInOwl:hasOBONamespace>
        <oboInOwl:id>GAZ:00076765</oboInOwl:id>
        <rdfs:label>Thuli Safari Area</rdfs:label>
    </owl:NamedIndividual>
    


    <!-- http://purl.obolibrary.org/obo/GAZ_00076766 -->

    <owl:NamedIndividual rdf:about="http://purl.obolibrary.org/obo/GAZ_00076766">
        <obo:RO_0001025 rdf:resource="http://purl.obolibrary.org/obo/GAZ_00076762"/>
        <oboInOwl:hasOBONamespace>GAZ</oboInOwl:hasOBONamespace>
        <oboInOwl:id>GAZ:00076766</oboInOwl:id>
        <rdfs:label>Tolo River Botanical Reserve</rdfs:label>
    </owl:NamedIndividual>
    


    <!-- http://purl.obolibrary.org/obo/GAZ_00132221 -->

    <owl:NamedIndividual rdf:about="http://purl.obolibrary.org/obo/GAZ_00132221">
        <obo:RO_0001025 rdf:resource="http://purl.obolibrary.org/obo/GAZ_00239405"/>
        <obo:IAO_0000115>A dam. Located 11 km S of Piggs Peak.</obo:IAO_0000115>
        <oboInOwl:hasOBONamespace>GAZ</oboInOwl:hasOBONamespace>
        <oboInOwl:id>GAZ:00132221</oboInOwl:id>
        <rdfs:label>Maguga Dam</rdfs:label>
    </owl:NamedIndividual>
    


    <!-- http://purl.obolibrary.org/obo/GAZ_00135239 -->

    <owl:NamedIndividual rdf:about="http://purl.obolibrary.org/obo/GAZ_00135239">
        <obo:IAO_0000115>A dam that forms a reservoir on the Mwenezi River in southern Zimbabwe. It is located in the Mwenezi District. Completed 1988.</obo:IAO_0000115>
        <oboInOwl:hasOBONamespace>GAZ</oboInOwl:hasOBONamespace>
        <oboInOwl:id>GAZ:00135239</oboInOwl:id>
        <rdfs:label>Manyuchi Dam</rdfs:label>
    </owl:NamedIndividual>
    


    <!-- http://purl.obolibrary.org/obo/GAZ_00143083 -->

    <owl:NamedIndividual rdf:about="http://purl.obolibrary.org/obo/GAZ_00143083">
        <obo:RO_0001025 rdf:resource="http://purl.obolibrary.org/obo/GAZ_00014117"/>
        <obo:IAO_0000115>The SW point of Marion Island.</obo:IAO_0000115>
        <oboInOwl:hasOBONamespace>GAZ</oboInOwl:hasOBONamespace>
        <oboInOwl:id>GAZ:00143083</oboInOwl:id>
        <rdfs:label>Cape Crozier</rdfs:label>
    </owl:NamedIndividual>
    


    <!-- http://purl.obolibrary.org/obo/GAZ_00143084 -->

    <owl:NamedIndividual rdf:about="http://purl.obolibrary.org/obo/GAZ_00143084">
        <obo:RO_0001025 rdf:resource="http://purl.obolibrary.org/obo/GAZ_00014117"/>
        <obo:IAO_0000115>The SE point of Marion Island.</obo:IAO_0000115>
        <oboInOwl:hasOBONamespace>GAZ</oboInOwl:hasOBONamespace>
        <oboInOwl:id>GAZ:00143084</oboInOwl:id>
        <rdfs:label>Cape Hooker</rdfs:label>
    </owl:NamedIndividual>
    


    <!-- http://purl.obolibrary.org/obo/GAZ_00143089 -->

    <owl:NamedIndividual rdf:about="http://purl.obolibrary.org/obo/GAZ_00143089">
        <obo:RO_0001025 rdf:resource="http://purl.obolibrary.org/obo/GAZ_00014117"/>
        <obo:IAO_0000115>The E point of Marion Island.</obo:IAO_0000115>
        <oboInOwl:hasOBONamespace>GAZ</oboInOwl:hasOBONamespace>
        <oboInOwl:id>GAZ:00143089</oboInOwl:id>
        <rdfs:label>East Cape</rdfs:label>
    </owl:NamedIndividual>
    


    <!-- http://purl.obolibrary.org/obo/GAZ_00143094 -->

    <owl:NamedIndividual rdf:about="http://purl.obolibrary.org/obo/GAZ_00143094">
        <obo:RO_0001025 rdf:resource="http://purl.obolibrary.org/obo/GAZ_00014117"/>
        <obo:IAO_0000115>The N point of Marion Island.</obo:IAO_0000115>
        <oboInOwl:hasOBONamespace>GAZ</oboInOwl:hasOBONamespace>
        <oboInOwl:id>GAZ:00143094</oboInOwl:id>
        <rdfs:label>Cape Davis</rdfs:label>
    </owl:NamedIndividual>
    


    <!-- http://purl.obolibrary.org/obo/GAZ_00143095 -->

    <owl:NamedIndividual rdf:about="http://purl.obolibrary.org/obo/GAZ_00143095">
        <obo:RO_0001025 rdf:resource="http://purl.obolibrary.org/obo/GAZ_00014117"/>
        <obo:IAO_0000115>A valley in SE Marion Island entering the Ocean just N of Kildalkey Bay.</obo:IAO_0000115>
        <oboInOwl:hasOBONamespace>GAZ</oboInOwl:hasOBONamespace>
        <oboInOwl:id>GAZ:00143095</oboInOwl:id>
        <rdfs:label>Black Haglet Valley</rdfs:label>
    </owl:NamedIndividual>
    


    <!-- http://purl.obolibrary.org/obo/GAZ_00143098 -->

    <owl:NamedIndividual rdf:about="http://purl.obolibrary.org/obo/GAZ_00143098">
        <obo:RO_0001025 rdf:resource="http://purl.obolibrary.org/obo/GAZ_00014118"/>
        <obo:IAO_0000115>The E point of Prince Edward Island.</obo:IAO_0000115>
        <oboInOwl:hasOBONamespace>GAZ</oboInOwl:hasOBONamespace>
        <oboInOwl:id>GAZ:00143098</oboInOwl:id>
        <rdfs:label>R.S.A Point</rdfs:label>
    </owl:NamedIndividual>
    


    <!-- http://purl.obolibrary.org/obo/GAZ_00143099 -->

    <owl:NamedIndividual rdf:about="http://purl.obolibrary.org/obo/GAZ_00143099">
        <obo:RO_0001025 rdf:resource="http://purl.obolibrary.org/obo/GAZ_00014118"/>
        <obo:IAO_0000115>A broad cape in the NW of Prince Edward Island.</obo:IAO_0000115>
        <oboInOwl:hasOBONamespace>GAZ</oboInOwl:hasOBONamespace>
        <oboInOwl:id>GAZ:00143099</oboInOwl:id>
        <rdfs:label>West Point</rdfs:label>
    </owl:NamedIndividual>
    


    <!-- http://purl.obolibrary.org/obo/GAZ_00143100 -->

    <owl:NamedIndividual rdf:about="http://purl.obolibrary.org/obo/GAZ_00143100">
        <obo:RO_0001025 rdf:resource="http://purl.obolibrary.org/obo/GAZ_00014118"/>
        <obo:IAO_0000115>The S point of Prince Edward Island.</obo:IAO_0000115>
        <oboInOwl:hasOBONamespace>GAZ</oboInOwl:hasOBONamespace>
        <oboInOwl:id>GAZ:00143100</oboInOwl:id>
        <rdfs:label>South Cape</rdfs:label>
    </owl:NamedIndividual>
    


    <!-- http://purl.obolibrary.org/obo/GAZ_00143101 -->

    <owl:NamedIndividual rdf:about="http://purl.obolibrary.org/obo/GAZ_00143101">
        <obo:RO_0001025 rdf:resource="http://purl.obolibrary.org/obo/GAZ_00014118"/>
        <obo:IAO_0000115>The SE point of Prince Edward Island.</obo:IAO_0000115>
        <oboInOwl:hasOBONamespace>GAZ</oboInOwl:hasOBONamespace>
        <oboInOwl:id>GAZ:00143101</oboInOwl:id>
        <rdfs:label>East Cape</rdfs:label>
    </owl:NamedIndividual>
    


    <!-- http://purl.obolibrary.org/obo/GAZ_00146342 -->

    <owl:NamedIndividual rdf:about="http://purl.obolibrary.org/obo/GAZ_00146342">
        <obo:RO_0001025 rdf:resource="http://purl.obolibrary.org/obo/GAZ_00002812"/>
        <obo:IAO_0000115>A 30 km2 lagoon of the Mhlatuze River, on the northern coast of KwaZulu-Natal.</obo:IAO_0000115>
        <oboInOwl:hasOBONamespace>GAZ</oboInOwl:hasOBONamespace>
        <oboInOwl:id>GAZ:00146342</oboInOwl:id>
        <rdfs:label>Richards Bay</rdfs:label>
    </owl:NamedIndividual>
    


    <!-- http://purl.obolibrary.org/obo/GAZ_00146589 -->

    <owl:NamedIndividual rdf:about="http://purl.obolibrary.org/obo/GAZ_00146589">
        <obo:RO_0001025 rdf:resource="http://purl.obolibrary.org/obo/GAZ_00076180"/>
        <obo:IAO_0000115>A group of 3 islands and some rocks in Algioa Bay. They lie in close proximity some 40 km east of the Saint Croix group or 53 km due east of Port Elizabeth and 7 km from the nearest landfall at Woody Cape.</obo:IAO_0000115>
        <oboInOwl:hasOBONamespace>GAZ</oboInOwl:hasOBONamespace>
        <oboInOwl:id>GAZ:00146589</oboInOwl:id>
        <rdfs:label>Bird Island Group</rdfs:label>
    </owl:NamedIndividual>
    


    <!-- http://purl.obolibrary.org/obo/GAZ_00146590 -->

    <owl:NamedIndividual rdf:about="http://purl.obolibrary.org/obo/GAZ_00146590">
        <rdf:type rdf:resource="http://purl.obolibrary.org/obo/ENVO_00000220"/>
        <obo:RO_0001025 rdf:resource="http://purl.obolibrary.org/obo/GAZ_00076180"/>
        <obo:IAO_0000115>An island group in Algoa Bay close inshore, near the new Ngquru harbour development at Coega, on the north-eastern outskirts of Port Elizabeth.</obo:IAO_0000115>
        <oboInOwl:hasOBONamespace>GAZ</oboInOwl:hasOBONamespace>
        <oboInOwl:id>GAZ:00146590</oboInOwl:id>
        <rdfs:label>Saint Croix Group</rdfs:label>
    </owl:NamedIndividual>
    


    <!-- http://purl.obolibrary.org/obo/GAZ_00146591 -->

    <owl:NamedIndividual rdf:about="http://purl.obolibrary.org/obo/GAZ_00146591">
        <obo:RO_0001025 rdf:resource="http://purl.obolibrary.org/obo/GAZ_00146590"/>
        <obo:IAO_0000115>An island just seaward to the Ngquru breakwater.</obo:IAO_0000115>
        <oboInOwl:hasOBONamespace>GAZ</oboInOwl:hasOBONamespace>
        <oboInOwl:id>GAZ:00146591</oboInOwl:id>
        <rdfs:label>Brenton Island</rdfs:label>
    </owl:NamedIndividual>
    


    <!-- http://purl.obolibrary.org/obo/GAZ_00146592 -->

    <owl:NamedIndividual rdf:about="http://purl.obolibrary.org/obo/GAZ_00146592">
        <obo:RO_0001025 rdf:resource="http://purl.obolibrary.org/obo/GAZ_00146590"/>
        <obo:IAO_0000115>The major of the Saint Croaix gorup of islands.</obo:IAO_0000115>
        <oboInOwl:hasOBONamespace>GAZ</oboInOwl:hasOBONamespace>
        <oboInOwl:id>GAZ:00146592</oboInOwl:id>
        <rdfs:label>Saint Croix Island</rdfs:label>
    </owl:NamedIndividual>
    


    <!-- http://purl.obolibrary.org/obo/GAZ_00146593 -->

    <owl:NamedIndividual rdf:about="http://purl.obolibrary.org/obo/GAZ_00146593">
        <obo:RO_0001025 rdf:resource="http://purl.obolibrary.org/obo/GAZ_00146590"/>
        <obo:IAO_0000115>An island just off the Ngquru breakwater.</obo:IAO_0000115>
        <oboInOwl:hasOBONamespace>GAZ</oboInOwl:hasOBONamespace>
        <oboInOwl:id>GAZ:00146593</oboInOwl:id>
        <rdfs:label>Jahleel Island</rdfs:label>
    </owl:NamedIndividual>
    


    <!-- http://purl.obolibrary.org/obo/GAZ_00146594 -->

    <owl:NamedIndividual rdf:about="http://purl.obolibrary.org/obo/GAZ_00146594">
        <obo:RO_0001025 rdf:resource="http://purl.obolibrary.org/obo/GAZ_00146589"/>
        <obo:IAO_0000115>One of the Bird Island Group.</obo:IAO_0000115>
        <oboInOwl:hasOBONamespace>GAZ</oboInOwl:hasOBONamespace>
        <oboInOwl:id>GAZ:00146594</oboInOwl:id>
        <rdfs:label>Stag Island</rdfs:label>
    </owl:NamedIndividual>
    


    <!-- http://purl.obolibrary.org/obo/GAZ_00146595 -->

    <owl:NamedIndividual rdf:about="http://purl.obolibrary.org/obo/GAZ_00146595">
        <obo:RO_0001025 rdf:resource="http://purl.obolibrary.org/obo/GAZ_00146589"/>
        <obo:IAO_0000115>One of the Bird Island Group.</obo:IAO_0000115>
        <oboInOwl:hasOBONamespace>GAZ</oboInOwl:hasOBONamespace>
        <oboInOwl:id>GAZ:00146595</oboInOwl:id>
        <rdfs:label>Seal Island</rdfs:label>
    </owl:NamedIndividual>
    


    <!-- http://purl.obolibrary.org/obo/GAZ_00146596 -->

    <owl:NamedIndividual rdf:about="http://purl.obolibrary.org/obo/GAZ_00146596">
        <obo:RO_0001025 rdf:resource="http://purl.obolibrary.org/obo/GAZ_00146589"/>
        <obo:IAO_0000115>One of the Bird Island Group.</obo:IAO_0000115>
        <oboInOwl:hasOBONamespace>GAZ</oboInOwl:hasOBONamespace>
        <oboInOwl:id>GAZ:00146596</oboInOwl:id>
        <rdfs:label>Bird Island</rdfs:label>
    </owl:NamedIndividual>
    


    <!-- http://purl.obolibrary.org/obo/GAZ_00146597 -->

    <owl:NamedIndividual rdf:about="http://purl.obolibrary.org/obo/GAZ_00146597">
        <obo:RO_0001025 rdf:resource="http://purl.obolibrary.org/obo/GAZ_00146589"/>
        <obo:IAO_0000115>A rock to the SW of the Bird Islands.</obo:IAO_0000115>
        <oboInOwl:hasOBONamespace>GAZ</oboInOwl:hasOBONamespace>
        <oboInOwl:id>GAZ:00146597</oboInOwl:id>
        <rdfs:label>Doddington Rock</rdfs:label>
    </owl:NamedIndividual>
    


    <!-- http://purl.obolibrary.org/obo/GAZ_00146598 -->

    <owl:NamedIndividual rdf:about="http://purl.obolibrary.org/obo/GAZ_00146598">
        <obo:RO_0001025 rdf:resource="http://purl.obolibrary.org/obo/GAZ_00146589"/>
        <obo:IAO_0000115>A rock to the SW of the Bird Islands.</obo:IAO_0000115>
        <oboInOwl:hasOBONamespace>GAZ</oboInOwl:hasOBONamespace>
        <oboInOwl:id>GAZ:00146598</oboInOwl:id>
        <rdfs:label>West Rock</rdfs:label>
    </owl:NamedIndividual>
    


    <!-- http://purl.obolibrary.org/obo/GAZ_00146599 -->

    <owl:NamedIndividual rdf:about="http://purl.obolibrary.org/obo/GAZ_00146599">
        <obo:RO_0001025 rdf:resource="http://purl.obolibrary.org/obo/GAZ_00146589"/>
        <obo:IAO_0000115>A rock to the SW of the Bird Islands.</obo:IAO_0000115>
        <oboInOwl:hasOBONamespace>GAZ</oboInOwl:hasOBONamespace>
        <oboInOwl:id>GAZ:00146599</oboInOwl:id>
        <rdfs:label>East Reef</rdfs:label>
    </owl:NamedIndividual>
    


    <!-- http://purl.obolibrary.org/obo/GAZ_00146601 -->

    <owl:NamedIndividual rdf:about="http://purl.obolibrary.org/obo/GAZ_00146601">
        <obo:RO_0001025 rdf:resource="http://purl.obolibrary.org/obo/GAZ_00076118"/>
        <obo:IAO_0000115>A natural harbour on the south-western coast of South Africa, north west of Cape Town.</obo:IAO_0000115>
        <oboInOwl:hasOBONamespace>GAZ</oboInOwl:hasOBONamespace>
        <oboInOwl:id>GAZ:00146601</oboInOwl:id>
        <rdfs:label>Saldanha Bay</rdfs:label>
    </owl:NamedIndividual>
    


    <!-- http://purl.obolibrary.org/obo/GAZ_00146602 -->

    <owl:NamedIndividual rdf:about="http://purl.obolibrary.org/obo/GAZ_00146602">
        <obo:RO_0001025 rdf:resource="http://purl.obolibrary.org/obo/GAZ_00076267"/>
        <obo:RO_0001025 rdf:resource="http://purl.obolibrary.org/obo/GAZ_00146601"/>
        <obo:IAO_0000115>A lagoon of Saldanha Bay.</obo:IAO_0000115>
        <oboInOwl:hasOBONamespace>GAZ</oboInOwl:hasOBONamespace>
        <oboInOwl:id>GAZ:00146602</oboInOwl:id>
        <rdfs:label>Langebaan Lagoon</rdfs:label>
    </owl:NamedIndividual>
    


    <!-- http://purl.obolibrary.org/obo/GAZ_00146603 -->

    <owl:NamedIndividual rdf:about="http://purl.obolibrary.org/obo/GAZ_00146603">
        <obo:RO_0001025 rdf:resource="http://purl.obolibrary.org/obo/GAZ_00005308"/>
        <obo:IAO_0000115>A wetland area.</obo:IAO_0000115>
        <oboInOwl:hasOBONamespace>GAZ</oboInOwl:hasOBONamespace>
        <oboInOwl:id>GAZ:00146603</oboInOwl:id>
        <rdfs:label>Mkhuze Swamp</rdfs:label>
    </owl:NamedIndividual>
    


    <!-- http://purl.obolibrary.org/obo/GAZ_00146604 -->

    <owl:NamedIndividual rdf:about="http://purl.obolibrary.org/obo/GAZ_00146604">
        <obo:RO_0001025 rdf:resource="http://purl.obolibrary.org/obo/GAZ_00005308"/>
        <obo:IAO_0000115>A wetland area.</obo:IAO_0000115>
        <oboInOwl:hasOBONamespace>GAZ</oboInOwl:hasOBONamespace>
        <oboInOwl:id>GAZ:00146604</oboInOwl:id>
        <rdfs:label>Umfolozi Swamp</rdfs:label>
    </owl:NamedIndividual>
    


    <!-- http://purl.obolibrary.org/obo/GAZ_00146606 -->

    <owl:NamedIndividual rdf:about="http://purl.obolibrary.org/obo/GAZ_00146606">
        <obo:RO_0001025 rdf:resource="http://purl.obolibrary.org/obo/GAZ_00076212"/>
        <obo:IAO_0000115>A lake in the Kosi System.</obo:IAO_0000115>
        <oboInOwl:hasOBONamespace>GAZ</oboInOwl:hasOBONamespace>
        <oboInOwl:id>GAZ:00146606</oboInOwl:id>
        <rdfs:label>Nhlange Lake</rdfs:label>
    </owl:NamedIndividual>
    


    <!-- http://purl.obolibrary.org/obo/GAZ_00146607 -->

    <owl:NamedIndividual rdf:about="http://purl.obolibrary.org/obo/GAZ_00146607">
        <obo:RO_0001025 rdf:resource="http://purl.obolibrary.org/obo/GAZ_00076212"/>
        <obo:IAO_0000115>A lake in the Kosi System.</obo:IAO_0000115>
        <oboInOwl:hasOBONamespace>GAZ</oboInOwl:hasOBONamespace>
        <oboInOwl:id>GAZ:00146607</oboInOwl:id>
        <rdfs:label>Amanzimnyama Lake</rdfs:label>
    </owl:NamedIndividual>
    


    <!-- http://purl.obolibrary.org/obo/GAZ_00146608 -->

    <owl:NamedIndividual rdf:about="http://purl.obolibrary.org/obo/GAZ_00146608">
        <obo:RO_0001025 rdf:resource="http://purl.obolibrary.org/obo/GAZ_00076212"/>
        <obo:IAO_0000115>A lake in the Kosi System.</obo:IAO_0000115>
        <oboInOwl:hasOBONamespace>GAZ</oboInOwl:hasOBONamespace>
        <oboInOwl:id>GAZ:00146608</oboInOwl:id>
        <rdfs:label>Makhawulani Lake</rdfs:label>
    </owl:NamedIndividual>
    


    <!-- http://purl.obolibrary.org/obo/GAZ_00146609 -->

    <owl:NamedIndividual rdf:about="http://purl.obolibrary.org/obo/GAZ_00146609">
        <obo:RO_0001025 rdf:resource="http://purl.obolibrary.org/obo/GAZ_00076212"/>
        <obo:IAO_0000115>The estuary beween First Lake and Kosi Mouth.</obo:IAO_0000115>
        <oboInOwl:hasOBONamespace>GAZ</oboInOwl:hasOBONamespace>
        <oboInOwl:id>GAZ:00146609</oboInOwl:id>
        <rdfs:label>Kosi Estuary</rdfs:label>
    </owl:NamedIndividual>
    


    <!-- http://purl.obolibrary.org/obo/GAZ_00146610 -->

    <owl:NamedIndividual rdf:about="http://purl.obolibrary.org/obo/GAZ_00146610">
        <obo:RO_0001025 rdf:resource="http://purl.obolibrary.org/obo/GAZ_00076212"/>
        <obo:IAO_0000115>The entrance of the Kosi Lake system to the Indian Ocean.</obo:IAO_0000115>
        <oboInOwl:hasOBONamespace>GAZ</oboInOwl:hasOBONamespace>
        <oboInOwl:id>GAZ:00146610</oboInOwl:id>
        <rdfs:label>Kosi Mouth</rdfs:label>
    </owl:NamedIndividual>
    


    <!-- http://purl.obolibrary.org/obo/GAZ_00146611 -->

    <owl:NamedIndividual rdf:about="http://purl.obolibrary.org/obo/GAZ_00146611">
        <obo:RO_0001025 rdf:resource="http://purl.obolibrary.org/obo/GAZ_00005308"/>
        <obo:IAO_0000115>A freshwater lake.</obo:IAO_0000115>
        <oboInOwl:hasOBONamespace>GAZ</oboInOwl:hasOBONamespace>
        <oboInOwl:id>GAZ:00146611</oboInOwl:id>
        <rdfs:label>Shengeza Lake</rdfs:label>
    </owl:NamedIndividual>
    


    <!-- http://purl.obolibrary.org/obo/GAZ_00146612 -->

    <owl:NamedIndividual rdf:about="http://purl.obolibrary.org/obo/GAZ_00146612">
        <obo:RO_0001025 rdf:resource="http://purl.obolibrary.org/obo/GAZ_00005308"/>
        <obo:IAO_0000115>A freshwater lake.</obo:IAO_0000115>
        <oboInOwl:hasOBONamespace>GAZ</oboInOwl:hasOBONamespace>
        <oboInOwl:id>GAZ:00146612</oboInOwl:id>
        <rdfs:label>Bhangazi South Lake</rdfs:label>
    </owl:NamedIndividual>
    


    <!-- http://purl.obolibrary.org/obo/GAZ_00146613 -->

    <owl:NamedIndividual rdf:about="http://purl.obolibrary.org/obo/GAZ_00146613">
        <obo:RO_0001025 rdf:resource="http://purl.obolibrary.org/obo/GAZ_00239837"/>
        <obo:IAO_0000115>A freshwater lake.</obo:IAO_0000115>
        <oboInOwl:hasOBONamespace>GAZ</oboInOwl:hasOBONamespace>
        <oboInOwl:id>GAZ:00146613</oboInOwl:id>
        <rdfs:label>Bhangazi North Lake</rdfs:label>
    </owl:NamedIndividual>
    


    <!-- http://purl.obolibrary.org/obo/GAZ_00146614 -->

    <owl:NamedIndividual rdf:about="http://purl.obolibrary.org/obo/GAZ_00146614">
        <obo:RO_0001025 rdf:resource="http://purl.obolibrary.org/obo/GAZ_00005308"/>
        <obo:IAO_0000115>A freshwater lake.</obo:IAO_0000115>
        <oboInOwl:hasOBONamespace>GAZ</oboInOwl:hasOBONamespace>
        <oboInOwl:id>GAZ:00146614</oboInOwl:id>
        <rdfs:label>Ngobezeleni Lake</rdfs:label>
    </owl:NamedIndividual>
    


    <!-- http://purl.obolibrary.org/obo/GAZ_00147073 -->

    <owl:NamedIndividual rdf:about="http://purl.obolibrary.org/obo/GAZ_00147073">
        <obo:RO_0001025 rdf:resource="http://purl.obolibrary.org/obo/GAZ_00009437"/>
        <obo:IAO_0000115>A generally rocky peninsula that juts out for 75 km into the Atlantic Ocean at the south-western extremity of the African continent. At the southern end of the peninsula are Cape Point and the Cape of Good Hope. On the northern end is the famous Table Mountain, overlooking Cape Town, South Africa.</obo:IAO_0000115>
        <oboInOwl:hasOBONamespace>GAZ</oboInOwl:hasOBONamespace>
        <oboInOwl:id>GAZ:00147073</oboInOwl:id>
        <rdfs:label>Cape Peninsula</rdfs:label>
    </owl:NamedIndividual>
    


    <!-- http://purl.obolibrary.org/obo/GAZ_00147074 -->

    <owl:NamedIndividual rdf:about="http://purl.obolibrary.org/obo/GAZ_00147074">
        <rdf:type rdf:resource="http://purl.obolibrary.org/obo/ENVO_00000305"/>
        <obo:RO_0001025 rdf:resource="http://purl.obolibrary.org/obo/GAZ_00076275"/>
        <obo:RO_0001025 rdf:resource="http://purl.obolibrary.org/obo/GAZ_00147073"/>
        <obo:IAO_0000115>A headland at the south-east corner of the Cape Peninsula. It is at the south-west corner of the Cape Peninsula, about 2.3 km west and a little south of Cape Point on the south-east corner.</obo:IAO_0000115>
        <oboInOwl:hasOBONamespace>GAZ</oboInOwl:hasOBONamespace>
        <oboInOwl:id>GAZ:00147074</oboInOwl:id>
        <rdfs:label>Cape Point</rdfs:label>
    </owl:NamedIndividual>
    


    <!-- http://purl.obolibrary.org/obo/GAZ_00147075 -->

    <owl:NamedIndividual rdf:about="http://purl.obolibrary.org/obo/GAZ_00147075">
        <obo:RO_0001025 rdf:resource="http://purl.obolibrary.org/obo/GAZ_00076275"/>
        <obo:RO_0001025 rdf:resource="http://purl.obolibrary.org/obo/GAZ_00147073"/>
        <obo:IAO_0000115>A rocky headland on the Atlantic coast of South Africa.</obo:IAO_0000115>
        <oboInOwl:hasOBONamespace>GAZ</oboInOwl:hasOBONamespace>
        <oboInOwl:id>GAZ:00147075</oboInOwl:id>
        <rdfs:label>Cape of Good Hope</rdfs:label>
    </owl:NamedIndividual>
    


    <!-- http://purl.obolibrary.org/obo/GAZ_00147076 -->

    <owl:NamedIndividual rdf:about="http://purl.obolibrary.org/obo/GAZ_00147076">
        <obo:RO_0001025 rdf:resource="http://purl.obolibrary.org/obo/GAZ_00076124"/>
        <obo:IAO_0000115>The geographic southern tip of the African continent. Located in the Overberg region, 170 km southeast of Cape Town. The cape is defined by the International Hydrographic Organization to be the dividing point between the Indian and Atlantic oceans.</obo:IAO_0000115>
        <oboInOwl:hasOBONamespace>GAZ</oboInOwl:hasOBONamespace>
        <oboInOwl:id>GAZ:00147076</oboInOwl:id>
        <rdfs:label>Cape Agulhas</rdfs:label>
    </owl:NamedIndividual>
    


    <!-- http://purl.obolibrary.org/obo/GAZ_00237426 -->

    <owl:NamedIndividual rdf:about="http://purl.obolibrary.org/obo/GAZ_00237426">
        <obo:RO_0001025 rdf:resource="http://purl.obolibrary.org/obo/GAZ_00076291"/>
        <obo:IAO_0000115>A large salt pan topographic depression which is part of the larger Makgadikgadi Pans in northeastern Botswana. This landform is a major part of the Nxai Pan National Park.</obo:IAO_0000115>
        <oboInOwl:hasOBONamespace>GAZ</oboInOwl:hasOBONamespace>
        <oboInOwl:id>GAZ:00237426</oboInOwl:id>
        <rdfs:label>Nxai Pan</rdfs:label>
    </owl:NamedIndividual>
    


    <!-- http://purl.obolibrary.org/obo/GAZ_00237427 -->

    <owl:NamedIndividual rdf:about="http://purl.obolibrary.org/obo/GAZ_00237427">
        <obo:RO_0001025 rdf:resource="http://purl.obolibrary.org/obo/GAZ_00075422"/>
        <obo:IAO_0000115>A large salt pan within the Makgadikgadi region of Botswana.</obo:IAO_0000115>
        <oboInOwl:hasOBONamespace>GAZ</oboInOwl:hasOBONamespace>
        <oboInOwl:id>GAZ:00237427</oboInOwl:id>
        <rdfs:label>Nwetwe Pan</rdfs:label>
    </owl:NamedIndividual>
    


    <!-- http://purl.obolibrary.org/obo/GAZ_00237428 -->

    <owl:NamedIndividual rdf:about="http://purl.obolibrary.org/obo/GAZ_00237428">
        <obo:RO_0001025 rdf:resource="http://purl.obolibrary.org/obo/GAZ_00075422"/>
        <obo:IAO_0000115>A large natural topographic depression within the Makgadikgadi region of Botswana. A seasonal lake.</obo:IAO_0000115>
        <oboInOwl:hasOBONamespace>GAZ</oboInOwl:hasOBONamespace>
        <oboInOwl:id>GAZ:00237428</oboInOwl:id>
        <rdfs:label>Sua Pan</rdfs:label>
    </owl:NamedIndividual>
    


    <!-- http://purl.obolibrary.org/obo/GAZ_00237596 -->

    <owl:NamedIndividual rdf:about="http://purl.obolibrary.org/obo/GAZ_00237596">
        <obo:IAO_0000115>A dam on the Shashe River near Francistown. Impounds Shashe Impoundment.</obo:IAO_0000115>
        <oboInOwl:hasOBONamespace>GAZ</oboInOwl:hasOBONamespace>
        <oboInOwl:id>GAZ:00237596</oboInOwl:id>
        <rdfs:label>Shashe Dam</rdfs:label>
    </owl:NamedIndividual>
    


    <!-- http://purl.obolibrary.org/obo/GAZ_00237597 -->

    <owl:NamedIndividual rdf:about="http://purl.obolibrary.org/obo/GAZ_00237597">
        <obo:IAO_0000115>A dam on the Thuli River, west of Gwanda, Zimbabwe. Impounds Thuli-Makwe Reservoir.</obo:IAO_0000115>
        <oboInOwl:hasOBONamespace>GAZ</oboInOwl:hasOBONamespace>
        <oboInOwl:id>GAZ:00237597</oboInOwl:id>
        <rdfs:label>Thuli-Makwe Dam</rdfs:label>
    </owl:NamedIndividual>
    


    <!-- http://purl.obolibrary.org/obo/GAZ_00237598 -->

    <owl:NamedIndividual rdf:about="http://purl.obolibrary.org/obo/GAZ_00237598">
        <obo:IAO_0000115>A reservoir. Impounded by Thuli-Makwe Dam.</obo:IAO_0000115>
        <oboInOwl:hasOBONamespace>GAZ</oboInOwl:hasOBONamespace>
        <oboInOwl:id>GAZ:00237598</oboInOwl:id>
        <rdfs:label>Thuli-Makwe Reservoir</rdfs:label>
    </owl:NamedIndividual>
    


    <!-- http://purl.obolibrary.org/obo/GAZ_00237602 -->

    <owl:NamedIndividual rdf:about="http://purl.obolibrary.org/obo/GAZ_00237602">
        <obo:IAO_0000115>A dam. Impounds Mtshabezi Reservoir.</obo:IAO_0000115>
        <oboInOwl:hasOBONamespace>GAZ</oboInOwl:hasOBONamespace>
        <oboInOwl:id>GAZ:00237602</oboInOwl:id>
        <rdfs:label>Mtshabezi Dam</rdfs:label>
    </owl:NamedIndividual>
    


    <!-- http://purl.obolibrary.org/obo/GAZ_00237603 -->

    <owl:NamedIndividual rdf:about="http://purl.obolibrary.org/obo/GAZ_00237603">
        <obo:IAO_0000115>A reservoir. Impounded by Mtshabezi Dam.</obo:IAO_0000115>
        <oboInOwl:hasOBONamespace>GAZ</oboInOwl:hasOBONamespace>
        <oboInOwl:id>GAZ:00237603</oboInOwl:id>
        <rdfs:label>Mtshabezi Reservoir</rdfs:label>
    </owl:NamedIndividual>
    


    <!-- http://purl.obolibrary.org/obo/GAZ_00237606 -->

    <owl:NamedIndividual rdf:about="http://purl.obolibrary.org/obo/GAZ_00237606">
        <obo:IAO_0000115>A river in southeastern Zimbabwe.</obo:IAO_0000115>
        <oboInOwl:hasOBONamespace>GAZ</oboInOwl:hasOBONamespace>
        <oboInOwl:id>GAZ:00237606</oboInOwl:id>
        <rdfs:label>Runde River</rdfs:label>
    </owl:NamedIndividual>
    


    <!-- http://purl.obolibrary.org/obo/GAZ_00237617 -->

    <owl:NamedIndividual rdf:about="http://purl.obolibrary.org/obo/GAZ_00237617">
        <obo:IAO_0000115>A river. A tributary of the Mzingwane River in Beitbridge District, Zimbabwe.</obo:IAO_0000115>
        <oboInOwl:hasOBONamespace>GAZ</oboInOwl:hasOBONamespace>
        <oboInOwl:id>GAZ:00237617</oboInOwl:id>
        <rdfs:label>Mtetengwe River</rdfs:label>
    </owl:NamedIndividual>
    


    <!-- http://purl.obolibrary.org/obo/GAZ_00237618 -->

    <owl:NamedIndividual rdf:about="http://purl.obolibrary.org/obo/GAZ_00237618">
        <obo:IAO_0000115>A dam. Located near the confluence with the Mzingwane River. Impounds Silalabuhwa Reservoir. Constructed 1966.</obo:IAO_0000115>
        <oboInOwl:hasOBONamespace>GAZ</oboInOwl:hasOBONamespace>
        <oboInOwl:id>GAZ:00237618</oboInOwl:id>
        <rdfs:label>Silalabuhwa Dam</rdfs:label>
    </owl:NamedIndividual>
    


    <!-- http://purl.obolibrary.org/obo/GAZ_00237619 -->

    <owl:NamedIndividual rdf:about="http://purl.obolibrary.org/obo/GAZ_00237619">
        <obo:IAO_0000115>A dam. Impounds Pangani Reservoir. Located near Filabusi.</obo:IAO_0000115>
        <oboInOwl:hasOBONamespace>GAZ</oboInOwl:hasOBONamespace>
        <oboInOwl:id>GAZ:00237619</oboInOwl:id>
        <rdfs:label>Pangani Dam</rdfs:label>
    </owl:NamedIndividual>
    


    <!-- http://purl.obolibrary.org/obo/GAZ_00237620 -->

    <owl:NamedIndividual rdf:about="http://purl.obolibrary.org/obo/GAZ_00237620">
        <obo:IAO_0000115>A dam. Impounds Insiza Reservoir. Constructed 1973.</obo:IAO_0000115>
        <oboInOwl:hasOBONamespace>GAZ</oboInOwl:hasOBONamespace>
        <oboInOwl:id>GAZ:00237620</oboInOwl:id>
        <rdfs:label>Insiza Dam</rdfs:label>
    </owl:NamedIndividual>
    


    <!-- http://purl.obolibrary.org/obo/GAZ_00237621 -->

    <owl:NamedIndividual rdf:about="http://purl.obolibrary.org/obo/GAZ_00237621">
        <obo:IAO_0000115>A dam. Located neat Fort Rixon. Impounds Upper Insiza Reservoir. Constructed 1967.</obo:IAO_0000115>
        <oboInOwl:hasOBONamespace>GAZ</oboInOwl:hasOBONamespace>
        <oboInOwl:id>GAZ:00237621</oboInOwl:id>
        <rdfs:label>Upper Insiza Dam</rdfs:label>
    </owl:NamedIndividual>
    


    <!-- http://purl.obolibrary.org/obo/GAZ_00237622 -->

    <owl:NamedIndividual rdf:about="http://purl.obolibrary.org/obo/GAZ_00237622">
        <obo:IAO_0000115>A reservoir. Impounded by Silalabuhwa Dam. Constructed 1966.</obo:IAO_0000115>
        <oboInOwl:hasOBONamespace>GAZ</oboInOwl:hasOBONamespace>
        <oboInOwl:id>GAZ:00237622</oboInOwl:id>
        <rdfs:label>Silalabuhwa Reservoir</rdfs:label>
    </owl:NamedIndividual>
    


    <!-- http://purl.obolibrary.org/obo/GAZ_00237623 -->

    <owl:NamedIndividual rdf:about="http://purl.obolibrary.org/obo/GAZ_00237623">
        <obo:IAO_0000115>A reservoir. Impounded by Pangani Dam.</obo:IAO_0000115>
        <oboInOwl:hasOBONamespace>GAZ</oboInOwl:hasOBONamespace>
        <oboInOwl:id>GAZ:00237623</oboInOwl:id>
        <rdfs:label>Pangani Reservoir</rdfs:label>
    </owl:NamedIndividual>
    


    <!-- http://purl.obolibrary.org/obo/GAZ_00237624 -->

    <owl:NamedIndividual rdf:about="http://purl.obolibrary.org/obo/GAZ_00237624">
        <obo:IAO_0000115>A reservoir. Impounded by Insiza Dam. Constructedf 1973.</obo:IAO_0000115>
        <oboInOwl:hasOBONamespace>GAZ</oboInOwl:hasOBONamespace>
        <oboInOwl:id>GAZ:00237624</oboInOwl:id>
        <rdfs:label>Insiza Reservoir</rdfs:label>
    </owl:NamedIndividual>
    


    <!-- http://purl.obolibrary.org/obo/GAZ_00237625 -->

    <owl:NamedIndividual rdf:about="http://purl.obolibrary.org/obo/GAZ_00237625">
        <obo:IAO_0000115>A reservoir. Impounded by Upper Insiza Dam. Constructed 1967.</obo:IAO_0000115>
        <oboInOwl:hasOBONamespace>GAZ</oboInOwl:hasOBONamespace>
        <oboInOwl:id>GAZ:00237625</oboInOwl:id>
        <rdfs:label>Upper Insiza Reservoir</rdfs:label>
    </owl:NamedIndividual>
    


    <!-- http://purl.obolibrary.org/obo/GAZ_00237626 -->

    <owl:NamedIndividual rdf:about="http://purl.obolibrary.org/obo/GAZ_00237626">
        <obo:IAO_0000115>A dam.</obo:IAO_0000115>
        <oboInOwl:hasOBONamespace>GAZ</oboInOwl:hasOBONamespace>
        <oboInOwl:id>GAZ:00237626</oboInOwl:id>
        <rdfs:label>Makado Dam</rdfs:label>
    </owl:NamedIndividual>
    


    <!-- http://purl.obolibrary.org/obo/GAZ_00237628 -->

    <owl:NamedIndividual rdf:about="http://purl.obolibrary.org/obo/GAZ_00237628">
        <obo:IAO_0000115>A dam.</obo:IAO_0000115>
        <oboInOwl:hasOBONamespace>GAZ</oboInOwl:hasOBONamespace>
        <oboInOwl:id>GAZ:00237628</oboInOwl:id>
        <rdfs:label>Tongwe Dam</rdfs:label>
    </owl:NamedIndividual>
    


    <!-- http://purl.obolibrary.org/obo/GAZ_00237629 -->

    <owl:NamedIndividual rdf:about="http://purl.obolibrary.org/obo/GAZ_00237629">
        <obo:IAO_0000115>A dam. Impounds Zhovhe Reservoir.</obo:IAO_0000115>
        <oboInOwl:hasOBONamespace>GAZ</oboInOwl:hasOBONamespace>
        <oboInOwl:id>GAZ:00237629</oboInOwl:id>
        <rdfs:label>Zhovhe Dam</rdfs:label>
    </owl:NamedIndividual>
    


    <!-- http://purl.obolibrary.org/obo/GAZ_00237630 -->

    <owl:NamedIndividual rdf:about="http://purl.obolibrary.org/obo/GAZ_00237630">
        <obo:IAO_0000115>A reservoir. Impounded by Zhovhe Dam.</obo:IAO_0000115>
        <oboInOwl:hasOBONamespace>GAZ</oboInOwl:hasOBONamespace>
        <oboInOwl:id>GAZ:00237630</oboInOwl:id>
        <rdfs:label>Zhovhe Reservoir</rdfs:label>
    </owl:NamedIndividual>
    


    <!-- http://purl.obolibrary.org/obo/GAZ_00237631 -->

    <owl:NamedIndividual rdf:about="http://purl.obolibrary.org/obo/GAZ_00237631">
        <obo:IAO_0000115>A river.</obo:IAO_0000115>
        <oboInOwl:hasOBONamespace>GAZ</oboInOwl:hasOBONamespace>
        <oboInOwl:id>GAZ:00237631</oboInOwl:id>
        <rdfs:label>Mutirikwe River</rdfs:label>
    </owl:NamedIndividual>
    


    <!-- http://purl.obolibrary.org/obo/GAZ_00238416 -->

    <owl:NamedIndividual rdf:about="http://purl.obolibrary.org/obo/GAZ_00238416">
        <obo:IAO_0000115>A lake located to the south of the Boteti River and the Makgadikgadi Pans, was once a large shallow lake fed by overspill from the Boteti River. However, since the impoundment at Mopipi, itself a former pan, the lake is usually as dry as the pans in nearby Makgadikgadi Depression.</obo:IAO_0000115>
        <oboInOwl:hasOBONamespace>GAZ</oboInOwl:hasOBONamespace>
        <oboInOwl:id>GAZ:00238416</oboInOwl:id>
        <rdfs:label>Lake Xau</rdfs:label>
    </owl:NamedIndividual>
    


    <!-- http://purl.obolibrary.org/obo/GAZ_00238674 -->

    <owl:NamedIndividual rdf:about="http://purl.obolibrary.org/obo/GAZ_00238674">
        <obo:IAO_0000115>A river.</obo:IAO_0000115>
        <oboInOwl:hasOBONamespace>GAZ</oboInOwl:hasOBONamespace>
        <oboInOwl:id>GAZ:00238674</oboInOwl:id>
        <rdfs:label>Notwane River</rdfs:label>
    </owl:NamedIndividual>
    


    <!-- http://purl.obolibrary.org/obo/GAZ_00238777 -->

    <owl:NamedIndividual rdf:about="http://purl.obolibrary.org/obo/GAZ_00238777">
        <obo:IAO_0000115>A headwater of the Nossob River.</obo:IAO_0000115>
        <oboInOwl:hasOBONamespace>GAZ</oboInOwl:hasOBONamespace>
        <oboInOwl:id>GAZ:00238777</oboInOwl:id>
        <rdfs:label>Swart-Nossob River</rdfs:label>
    </owl:NamedIndividual>
    


    <!-- http://purl.obolibrary.org/obo/GAZ_00238778 -->

    <owl:NamedIndividual rdf:about="http://purl.obolibrary.org/obo/GAZ_00238778">
        <obo:IAO_0000115>A headwater of the Nossob River.</obo:IAO_0000115>
        <oboInOwl:hasOBONamespace>GAZ</oboInOwl:hasOBONamespace>
        <oboInOwl:id>GAZ:00238778</oboInOwl:id>
        <rdfs:label>Wit-Nossob River</rdfs:label>
    </owl:NamedIndividual>
    


    <!-- http://purl.obolibrary.org/obo/GAZ_00238779 -->

    <owl:NamedIndividual rdf:about="http://purl.obolibrary.org/obo/GAZ_00238779">
        <obo:IAO_0000115>A river. A tributary of the Nossob River.</obo:IAO_0000115>
        <oboInOwl:hasOBONamespace>GAZ</oboInOwl:hasOBONamespace>
        <oboInOwl:id>GAZ:00238779</oboInOwl:id>
        <rdfs:label>Auob River</rdfs:label>
    </owl:NamedIndividual>
    


    <!-- http://purl.obolibrary.org/obo/GAZ_00238782 -->

    <owl:NamedIndividual rdf:about="http://purl.obolibrary.org/obo/GAZ_00238782">
        <obo:RO_0001025 rdf:resource="http://purl.obolibrary.org/obo/GAZ_00237428"/>
        <obo:IAO_0000115>An igneous rock island in Sua Pan.</obo:IAO_0000115>
        <oboInOwl:hasOBONamespace>GAZ</oboInOwl:hasOBONamespace>
        <oboInOwl:id>GAZ:00238782</oboInOwl:id>
        <rdfs:label>Kukome Island</rdfs:label>
    </owl:NamedIndividual>
    


    <!-- http://purl.obolibrary.org/obo/GAZ_00238901 -->

    <owl:NamedIndividual rdf:about="http://purl.obolibrary.org/obo/GAZ_00238901">
        <obo:IAO_0000115>Pans located SW of the Makgadikgadi Pans.</obo:IAO_0000115>
        <oboInOwl:hasOBONamespace>GAZ</oboInOwl:hasOBONamespace>
        <oboInOwl:id>GAZ:00238901</oboInOwl:id>
        <rdfs:label>Deception Pans</rdfs:label>
    </owl:NamedIndividual>
    


    <!-- http://purl.obolibrary.org/obo/GAZ_00238904 -->

    <owl:NamedIndividual rdf:about="http://purl.obolibrary.org/obo/GAZ_00238904">
        <obo:IAO_0000115>A dam.</obo:IAO_0000115>
        <oboInOwl:hasOBONamespace>GAZ</oboInOwl:hasOBONamespace>
        <oboInOwl:id>GAZ:00238904</oboInOwl:id>
        <rdfs:label>Muela Dam</rdfs:label>
    </owl:NamedIndividual>
    


    <!-- http://purl.obolibrary.org/obo/GAZ_00238915 -->

    <owl:NamedIndividual rdf:about="http://purl.obolibrary.org/obo/GAZ_00238915">
        <obo:IAO_0000115>A river in northern Lesotho. It flows south from close to the South African border, past the town of Ha Lejone and joins the Senqu River close to the town of Taung.</obo:IAO_0000115>
        <oboInOwl:hasOBONamespace>GAZ</oboInOwl:hasOBONamespace>
        <oboInOwl:id>GAZ:00238915</oboInOwl:id>
        <rdfs:label>Malibamat&apos;so River</rdfs:label>
    </owl:NamedIndividual>
    


    <!-- http://purl.obolibrary.org/obo/GAZ_00239404 -->

    <owl:NamedIndividual rdf:about="http://purl.obolibrary.org/obo/GAZ_00239404">
        <rdf:type rdf:resource="http://purl.obolibrary.org/obo/ENVO_00000856"/>
        <obo:RO_0001025 rdf:resource="http://purl.obolibrary.org/obo/GAZ_00032885"/>
        <obo:IAO_0000115>A populated place. A town.</obo:IAO_0000115>
        <oboInOwl:hasOBONamespace>GAZ</oboInOwl:hasOBONamespace>
        <oboInOwl:id>GAZ:00239404</oboInOwl:id>
        <rdfs:label>Ermelo</rdfs:label>
    </owl:NamedIndividual>
    


    <!-- http://purl.obolibrary.org/obo/GAZ_00239405 -->

    <owl:NamedIndividual rdf:about="http://purl.obolibrary.org/obo/GAZ_00239405">
        <obo:RO_0001025 rdf:resource="http://purl.obolibrary.org/obo/GAZ_00032885"/>
        <obo:IAO_0000115>A river in South Africa, Swaziland and Mozambique. The river rises at an elevation of about 5,000 feet near Breyten in the Ermelo district of the Mpumalanga province. It flows in a general northeasterly direction and reaches the Indian Ocean at Maputo Bay, after a course of some 480 km.</obo:IAO_0000115>
        <oboInOwl:hasOBONamespace>GAZ</oboInOwl:hasOBONamespace>
        <oboInOwl:id>GAZ:00239405</oboInOwl:id>
        <rdfs:label>Komati River</rdfs:label>
    </owl:NamedIndividual>
    


    <!-- http://purl.obolibrary.org/obo/GAZ_00239406 -->

    <owl:NamedIndividual rdf:about="http://purl.obolibrary.org/obo/GAZ_00239406">
        <obo:RO_0001025 rdf:resource="http://purl.obolibrary.org/obo/GAZ_00002816"/>
        <obo:IAO_0000115>A river valley in the Mpumalanga Province in central South Africa.</obo:IAO_0000115>
        <oboInOwl:hasOBONamespace>GAZ</oboInOwl:hasOBONamespace>
        <oboInOwl:id>GAZ:00239406</oboInOwl:id>
        <rdfs:label>Komati Gorge</rdfs:label>
    </owl:NamedIndividual>
    


    <!-- http://purl.obolibrary.org/obo/GAZ_00239411 -->

    <owl:NamedIndividual rdf:about="http://purl.obolibrary.org/obo/GAZ_00239411">
        <obo:RO_0001025 rdf:resource="http://purl.obolibrary.org/obo/GAZ_00002816"/>
        <obo:IAO_0000115>A populated place. A town situated at the confluence of the Crocodile and Komati Rivers in Mpumalanga province, South Africa.</obo:IAO_0000115>
        <oboInOwl:hasOBONamespace>GAZ</oboInOwl:hasOBONamespace>
        <oboInOwl:id>GAZ:00239411</oboInOwl:id>
        <rdfs:label>Komatipoort</rdfs:label>
    </owl:NamedIndividual>
    


    <!-- http://purl.obolibrary.org/obo/GAZ_00239442 -->

    <owl:NamedIndividual rdf:about="http://purl.obolibrary.org/obo/GAZ_00239442">
        <obo:IAO_0000115>A dam close to Mariental, Hardap Region, Namibia.</obo:IAO_0000115>
        <oboInOwl:hasOBONamespace>GAZ</oboInOwl:hasOBONamespace>
        <oboInOwl:id>GAZ:00239442</oboInOwl:id>
        <rdfs:label>Hardap Dam</rdfs:label>
    </owl:NamedIndividual>
    


    <!-- http://purl.obolibrary.org/obo/GAZ_00239490 -->

    <owl:NamedIndividual rdf:about="http://purl.obolibrary.org/obo/GAZ_00239490">
        <obo:IAO_0000115>A river. A tributary of the Fish River.</obo:IAO_0000115>
        <oboInOwl:hasOBONamespace>GAZ</oboInOwl:hasOBONamespace>
        <oboInOwl:id>GAZ:00239490</oboInOwl:id>
        <rdfs:label>Lowen River</rdfs:label>
    </owl:NamedIndividual>
    


    <!-- http://purl.obolibrary.org/obo/GAZ_00239491 -->

    <owl:NamedIndividual rdf:about="http://purl.obolibrary.org/obo/GAZ_00239491">
        <obo:RO_0001025 rdf:resource="http://purl.obolibrary.org/obo/GAZ_00239490"/>
        <obo:IAO_0000115>A dam outside of Keetmanshoop, Karas Region, Namibia. Impounds Naute Reservoir. Completed 1972-09.</obo:IAO_0000115>
        <oboInOwl:hasOBONamespace>GAZ</oboInOwl:hasOBONamespace>
        <oboInOwl:id>GAZ:00239491</oboInOwl:id>
        <rdfs:label>Naute Dam</rdfs:label>
    </owl:NamedIndividual>
    


    <!-- http://purl.obolibrary.org/obo/GAZ_00239524 -->

    <owl:NamedIndividual rdf:about="http://purl.obolibrary.org/obo/GAZ_00239524">
        <obo:RO_0001025 rdf:resource="http://purl.obolibrary.org/obo/GAZ_00076641"/>
        <obo:IAO_0000115>Sulfurous hot springs.</obo:IAO_0000115>
        <oboInOwl:hasOBONamespace>GAZ</oboInOwl:hasOBONamespace>
        <oboInOwl:id>GAZ:00239524</oboInOwl:id>
        <rdfs:label>Ai-Ais Hot Springs</rdfs:label>
    </owl:NamedIndividual>
    


    <!-- http://purl.obolibrary.org/obo/GAZ_00239536 -->

    <owl:NamedIndividual rdf:about="http://purl.obolibrary.org/obo/GAZ_00239536">
        <obo:RO_0001025 rdf:resource="http://purl.obolibrary.org/obo/GAZ_00239405"/>
        <obo:IAO_0000115>A reservoir. Impounded by Maguga Dam.</obo:IAO_0000115>
        <oboInOwl:hasOBONamespace>GAZ</oboInOwl:hasOBONamespace>
        <oboInOwl:id>GAZ:00239536</oboInOwl:id>
        <rdfs:label>Maguga Reservoir</rdfs:label>
    </owl:NamedIndividual>
    


    <!-- http://purl.obolibrary.org/obo/GAZ_00239541 -->

    <owl:NamedIndividual rdf:about="http://purl.obolibrary.org/obo/GAZ_00239541">
        <obo:RO_0001025 rdf:resource="http://purl.obolibrary.org/obo/GAZ_00012792"/>
        <obo:IAO_0000115>A national park in the Garden Route region of South Africa. It was established by amalgamating the existing Tsitsikamma and Wilderness National Parks, the Knysna National Lake Area, and various other areas of state-owned land. Established 2009-03-06.</obo:IAO_0000115>
        <oboInOwl:hasOBONamespace>GAZ</oboInOwl:hasOBONamespace>
        <oboInOwl:id>GAZ:00239541</oboInOwl:id>
        <rdfs:label>Garden Route National Park</rdfs:label>
    </owl:NamedIndividual>
    


    <!-- http://purl.obolibrary.org/obo/GAZ_00239542 -->

    <owl:NamedIndividual rdf:about="http://purl.obolibrary.org/obo/GAZ_00239542">
        <obo:RO_0001025 rdf:resource="http://purl.obolibrary.org/obo/GAZ_00239541"/>
        <obo:IAO_0000115>A lagoon at the mouth of the Knysna River.</obo:IAO_0000115>
        <oboInOwl:hasOBONamespace>GAZ</oboInOwl:hasOBONamespace>
        <oboInOwl:id>GAZ:00239542</oboInOwl:id>
        <rdfs:label>Knysna Lagoon</rdfs:label>
    </owl:NamedIndividual>
    


    <!-- http://purl.obolibrary.org/obo/GAZ_00239543 -->

    <owl:NamedIndividual rdf:about="http://purl.obolibrary.org/obo/GAZ_00239543">
        <obo:RO_0001025 rdf:resource="http://purl.obolibrary.org/obo/GAZ_00002819"/>
        <obo:IAO_0000115>A river in the Eastern Cape province of South Africa. The river mouth is located in the Tsitsikamma National Park.</obo:IAO_0000115>
        <oboInOwl:hasOBONamespace>GAZ</oboInOwl:hasOBONamespace>
        <oboInOwl:id>GAZ:00239543</oboInOwl:id>
        <rdfs:label>Storms River</rdfs:label>
    </owl:NamedIndividual>
    


    <!-- http://purl.obolibrary.org/obo/GAZ_00239545 -->

    <owl:NamedIndividual rdf:about="http://purl.obolibrary.org/obo/GAZ_00239545">
        <obo:RO_0001025 rdf:resource="http://purl.obolibrary.org/obo/GAZ_00002819"/>
        <obo:IAO_0000115>A river situated in the city of East London on the East Coast of South Africa. It is to the west of the Nahoon River. The town of East London was established around it.</obo:IAO_0000115>
        <oboInOwl:hasOBONamespace>GAZ</oboInOwl:hasOBONamespace>
        <oboInOwl:id>GAZ:00239545</oboInOwl:id>
        <rdfs:label>Buffalo River</rdfs:label>
    </owl:NamedIndividual>
    


    <!-- http://purl.obolibrary.org/obo/GAZ_00239546 -->

    <owl:NamedIndividual rdf:about="http://purl.obolibrary.org/obo/GAZ_00239546">
        <obo:RO_0001025 rdf:resource="http://purl.obolibrary.org/obo/GAZ_00075958"/>
        <obo:IAO_0000115>A city. It lies on the Indian Ocean coast, largely between the Buffalo River and the Nahoon River.</obo:IAO_0000115>
        <oboInOwl:hasOBONamespace>GAZ</oboInOwl:hasOBONamespace>
        <oboInOwl:id>GAZ:00239546</oboInOwl:id>
        <rdfs:label>East London</rdfs:label>
    </owl:NamedIndividual>
    


    <!-- http://purl.obolibrary.org/obo/GAZ_00239547 -->

    <owl:NamedIndividual rdf:about="http://purl.obolibrary.org/obo/GAZ_00239547">
        <obo:RO_0001025 rdf:resource="http://purl.obolibrary.org/obo/GAZ_00002819"/>
        <obo:IAO_0000115>A river situated in the city East London on the East Coast of South Africa.</obo:IAO_0000115>
        <oboInOwl:hasOBONamespace>GAZ</oboInOwl:hasOBONamespace>
        <oboInOwl:id>GAZ:00239547</oboInOwl:id>
        <rdfs:label>Nahoon River</rdfs:label>
    </owl:NamedIndividual>
    


    <!-- http://purl.obolibrary.org/obo/GAZ_00239548 -->

    <owl:NamedIndividual rdf:about="http://purl.obolibrary.org/obo/GAZ_00239548">
        <obo:RO_0001025 rdf:resource="http://purl.obolibrary.org/obo/GAZ_00239547"/>
        <obo:IAO_0000115>A dam.</obo:IAO_0000115>
        <oboInOwl:hasOBONamespace>GAZ</oboInOwl:hasOBONamespace>
        <oboInOwl:id>GAZ:00239548</oboInOwl:id>
        <rdfs:label>Nahoon Dam</rdfs:label>
    </owl:NamedIndividual>
    


    <!-- http://purl.obolibrary.org/obo/GAZ_00239549 -->

    <owl:NamedIndividual rdf:about="http://purl.obolibrary.org/obo/GAZ_00239549">
        <obo:RO_0001025 rdf:resource="http://purl.obolibrary.org/obo/GAZ_00032858"/>
        <obo:IAO_0000115>A protected area. Established 2005-10-30.</obo:IAO_0000115>
        <oboInOwl:hasOBONamespace>GAZ</oboInOwl:hasOBONamespace>
        <oboInOwl:id>GAZ:00239549</oboInOwl:id>
        <rdfs:label>Camdeboo National Park</rdfs:label>
    </owl:NamedIndividual>
    


    <!-- http://purl.obolibrary.org/obo/GAZ_00239550 -->

    <owl:NamedIndividual rdf:about="http://purl.obolibrary.org/obo/GAZ_00239550">
        <obo:RO_0001025 rdf:resource="http://purl.obolibrary.org/obo/GAZ_00002819"/>
        <obo:IAO_0000115>A river located in the Eastern Cape Province of South Africa. It discharges to the Indian Ocean between Jeffreys Bay and Port Elizabeth.</obo:IAO_0000115>
        <oboInOwl:hasOBONamespace>GAZ</oboInOwl:hasOBONamespace>
        <oboInOwl:id>GAZ:00239550</oboInOwl:id>
        <rdfs:label>Gamtoos River</rdfs:label>
    </owl:NamedIndividual>
    


    <!-- http://purl.obolibrary.org/obo/GAZ_00239551 -->

    <owl:NamedIndividual rdf:about="http://purl.obolibrary.org/obo/GAZ_00239551">
        <obo:RO_0001025 rdf:resource="http://purl.obolibrary.org/obo/GAZ_00002819"/>
        <obo:IAO_0000115>A river in South Africa in the Eastern Cape province. It flows for 520 km and ends at the Indian Ocean with the small town Kei Mouth on the west bank. The river serves as the southwestern border of the Transkei region.</obo:IAO_0000115>
        <oboInOwl:hasOBONamespace>GAZ</oboInOwl:hasOBONamespace>
        <oboInOwl:id>GAZ:00239551</oboInOwl:id>
        <rdfs:label>Great Kei River</rdfs:label>
    </owl:NamedIndividual>
    


    <!-- http://purl.obolibrary.org/obo/GAZ_00239552 -->

    <owl:NamedIndividual rdf:about="http://purl.obolibrary.org/obo/GAZ_00239552">
        <obo:RO_0001025 rdf:resource="http://purl.obolibrary.org/obo/GAZ_00076131"/>
        <obo:IAO_0000115>A river in the Eastern Cape and Western Cape provinces of South Africa. Discharges to the Indian Ocean at Nature&apos;s Valley.</obo:IAO_0000115>
        <oboInOwl:hasOBONamespace>GAZ</oboInOwl:hasOBONamespace>
        <oboInOwl:id>GAZ:00239552</oboInOwl:id>
        <rdfs:label>Groot River</rdfs:label>
    </owl:NamedIndividual>
    


    <!-- http://purl.obolibrary.org/obo/GAZ_00239553 -->

    <owl:NamedIndividual rdf:about="http://purl.obolibrary.org/obo/GAZ_00239553">
        <obo:RO_0001025 rdf:resource="http://purl.obolibrary.org/obo/GAZ_00075956"/>
        <obo:IAO_0000115>A series of caves located to the east of the Klasies River mouth on the Tsitsikamma coast in the Humansdorp district of Eastern Cape Province, South Africa. An archeological site. The five caves are dotted eastwards along the coast within 2 km of Klasies River mouth, and the complete stretch to Druipkelder Point is designated as a National Monument and a Natural Heritage Area.</obo:IAO_0000115>
        <oboInOwl:hasOBONamespace>GAZ</oboInOwl:hasOBONamespace>
        <oboInOwl:id>GAZ:00239553</oboInOwl:id>
        <rdfs:label>Klasies River Caves</rdfs:label>
    </owl:NamedIndividual>
    


    <!-- http://purl.obolibrary.org/obo/GAZ_00239554 -->

    <owl:NamedIndividual rdf:about="http://purl.obolibrary.org/obo/GAZ_00239554">
        <obo:RO_0001025 rdf:resource="http://purl.obolibrary.org/obo/GAZ_00239553"/>
        <obo:IAO_0000115>A cave.</obo:IAO_0000115>
        <oboInOwl:hasOBONamespace>GAZ</oboInOwl:hasOBONamespace>
        <oboInOwl:id>GAZ:00239554</oboInOwl:id>
        <rdfs:label>Klasies Main Site</rdfs:label>
    </owl:NamedIndividual>
    


    <!-- http://purl.obolibrary.org/obo/GAZ_00239555 -->

    <owl:NamedIndividual rdf:about="http://purl.obolibrary.org/obo/GAZ_00239555">
        <obo:RO_0001025 rdf:resource="http://purl.obolibrary.org/obo/GAZ_00239554"/>
        <obo:IAO_0000115>A cave.</obo:IAO_0000115>
        <oboInOwl:hasOBONamespace>GAZ</oboInOwl:hasOBONamespace>
        <oboInOwl:id>GAZ:00239555</oboInOwl:id>
        <rdfs:label>Klasies Cave 1</rdfs:label>
    </owl:NamedIndividual>
    


    <!-- http://purl.obolibrary.org/obo/GAZ_00239556 -->

    <owl:NamedIndividual rdf:about="http://purl.obolibrary.org/obo/GAZ_00239556">
        <obo:RO_0001025 rdf:resource="http://purl.obolibrary.org/obo/GAZ_00239554"/>
        <obo:IAO_0000115>A cave.</obo:IAO_0000115>
        <oboInOwl:hasOBONamespace>GAZ</oboInOwl:hasOBONamespace>
        <oboInOwl:id>GAZ:00239556</oboInOwl:id>
        <rdfs:label>Klasies Cave 2</rdfs:label>
    </owl:NamedIndividual>
    


    <!-- http://purl.obolibrary.org/obo/GAZ_00239557 -->

    <owl:NamedIndividual rdf:about="http://purl.obolibrary.org/obo/GAZ_00239557">
        <obo:RO_0001025 rdf:resource="http://purl.obolibrary.org/obo/GAZ_00239553"/>
        <obo:IAO_0000115>A cave.</obo:IAO_0000115>
        <oboInOwl:hasOBONamespace>GAZ</oboInOwl:hasOBONamespace>
        <oboInOwl:id>GAZ:00239557</oboInOwl:id>
        <rdfs:label>Klasies Cave 3</rdfs:label>
    </owl:NamedIndividual>
    


    <!-- http://purl.obolibrary.org/obo/GAZ_00239558 -->

    <owl:NamedIndividual rdf:about="http://purl.obolibrary.org/obo/GAZ_00239558">
        <obo:RO_0001025 rdf:resource="http://purl.obolibrary.org/obo/GAZ_00239553"/>
        <obo:IAO_0000115>A cave.</obo:IAO_0000115>
        <oboInOwl:hasOBONamespace>GAZ</oboInOwl:hasOBONamespace>
        <oboInOwl:id>GAZ:00239558</oboInOwl:id>
        <rdfs:label>Klasies Cave 4</rdfs:label>
    </owl:NamedIndividual>
    


    <!-- http://purl.obolibrary.org/obo/GAZ_00239559 -->

    <owl:NamedIndividual rdf:about="http://purl.obolibrary.org/obo/GAZ_00239559">
        <obo:RO_0001025 rdf:resource="http://purl.obolibrary.org/obo/GAZ_00239553"/>
        <obo:IAO_0000115>A cave.</obo:IAO_0000115>
        <oboInOwl:hasOBONamespace>GAZ</oboInOwl:hasOBONamespace>
        <oboInOwl:id>GAZ:00239559</oboInOwl:id>
        <rdfs:label>Klasies Cave 5</rdfs:label>
    </owl:NamedIndividual>
    


    <!-- http://purl.obolibrary.org/obo/GAZ_00239561 -->

    <owl:NamedIndividual rdf:about="http://purl.obolibrary.org/obo/GAZ_00239561">
        <obo:RO_0001025 rdf:resource="http://purl.obolibrary.org/obo/GAZ_00002819"/>
        <obo:IAO_0000115>A river in the Eastern Cape Province of South Africa. Its source is in the Compassberg Mountains near Nieu-Bethesda. The river then flows in a general southsoutheasterly direction, passing the town Graaff-Reinet in the Karoo before winding its way through the Zuurberg Mountains and then past Kirkwood and Addo in the fertile Sundays River Valley. It empties into the Indian Ocean at Algoa Bay after running through the village of Colchester, 40 km east of the city of Port Elizabeth.</obo:IAO_0000115>
        <oboInOwl:hasOBONamespace>GAZ</oboInOwl:hasOBONamespace>
        <oboInOwl:id>GAZ:00239561</oboInOwl:id>
        <rdfs:label>Sundays River</rdfs:label>
    </owl:NamedIndividual>
    


    <!-- http://purl.obolibrary.org/obo/GAZ_00239562 -->

    <owl:NamedIndividual rdf:about="http://purl.obolibrary.org/obo/GAZ_00239562">
        <rdf:type rdf:resource="http://purl.obolibrary.org/obo/ENVO_00000856"/>
        <obo:RO_0001025 rdf:resource="http://purl.obolibrary.org/obo/GAZ_00032858"/>
        <obo:IAO_0000115>A populated place. A town.</obo:IAO_0000115>
        <oboInOwl:hasOBONamespace>GAZ</oboInOwl:hasOBONamespace>
        <oboInOwl:id>GAZ:00239562</oboInOwl:id>
        <rdfs:label>Graaff Reinet</rdfs:label>
    </owl:NamedIndividual>
    


    <!-- http://purl.obolibrary.org/obo/GAZ_00239563 -->

    <owl:NamedIndividual rdf:about="http://purl.obolibrary.org/obo/GAZ_00239563">
        <obo:RO_0001025 rdf:resource="http://purl.obolibrary.org/obo/GAZ_00032858"/>
        <obo:IAO_0000115>A river in the Eastern Cape province of South Africa. The river mouth is located about 30 km west of Port Elizabeth.</obo:IAO_0000115>
        <oboInOwl:hasOBONamespace>GAZ</oboInOwl:hasOBONamespace>
        <oboInOwl:id>GAZ:00239563</oboInOwl:id>
        <rdfs:label>Van Stadens River</rdfs:label>
    </owl:NamedIndividual>
    


    <!-- http://purl.obolibrary.org/obo/GAZ_00239564 -->

    <owl:NamedIndividual rdf:about="http://purl.obolibrary.org/obo/GAZ_00239564">
        <rdf:type rdf:resource="http://purl.obolibrary.org/obo/ENVO_00000856"/>
        <obo:RO_0001025 rdf:resource="http://purl.obolibrary.org/obo/GAZ_00075955"/>
        <obo:IAO_0000115>A populated place. A town.</obo:IAO_0000115>
        <oboInOwl:hasOBONamespace>GAZ</oboInOwl:hasOBONamespace>
        <oboInOwl:id>GAZ:00239564</oboInOwl:id>
        <rdfs:label>Kirkwood</rdfs:label>
    </owl:NamedIndividual>
    


    <!-- http://purl.obolibrary.org/obo/GAZ_00239565 -->

    <owl:NamedIndividual rdf:about="http://purl.obolibrary.org/obo/GAZ_00239565">
        <obo:RO_0001025 rdf:resource="http://purl.obolibrary.org/obo/GAZ_00075951"/>
        <obo:IAO_0000115>A protected area along the Kowie River.</obo:IAO_0000115>
        <oboInOwl:hasOBONamespace>GAZ</oboInOwl:hasOBONamespace>
        <oboInOwl:id>GAZ:00239565</oboInOwl:id>
        <rdfs:label>Waters Meeting Nature Reserve</rdfs:label>
    </owl:NamedIndividual>
    


    <!-- http://purl.obolibrary.org/obo/GAZ_00239566 -->

    <owl:NamedIndividual rdf:about="http://purl.obolibrary.org/obo/GAZ_00239566">
        <obo:RO_0001025 rdf:resource="http://purl.obolibrary.org/obo/GAZ_00002819"/>
        <obo:IAO_0000115>A river.</obo:IAO_0000115>
        <oboInOwl:hasOBONamespace>GAZ</oboInOwl:hasOBONamespace>
        <oboInOwl:id>GAZ:00239566</oboInOwl:id>
        <rdfs:label>Kowie River</rdfs:label>
    </owl:NamedIndividual>
    


    <!-- http://purl.obolibrary.org/obo/GAZ_00239571 -->

    <owl:NamedIndividual rdf:about="http://purl.obolibrary.org/obo/GAZ_00239571">
        <obo:RO_0001025 rdf:resource="http://purl.obolibrary.org/obo/GAZ_00076190"/>
        <obo:IAO_0000115>A reservoir.</obo:IAO_0000115>
        <oboInOwl:hasOBONamespace>GAZ</oboInOwl:hasOBONamespace>
        <oboInOwl:id>GAZ:00239571</oboInOwl:id>
        <rdfs:label>Commando Drift Dam Reservoir</rdfs:label>
    </owl:NamedIndividual>
    


    <!-- http://purl.obolibrary.org/obo/GAZ_00239572 -->

    <owl:NamedIndividual rdf:about="http://purl.obolibrary.org/obo/GAZ_00239572">
        <obo:IAO_0000115>A reservoir. Impounded by Gariep Dam. Completed 1971.</obo:IAO_0000115>
        <oboInOwl:hasOBONamespace>GAZ</oboInOwl:hasOBONamespace>
        <oboInOwl:id>GAZ:00239572</oboInOwl:id>
        <rdfs:label>Lake Gariep</rdfs:label>
    </owl:NamedIndividual>
    


    <!-- http://purl.obolibrary.org/obo/GAZ_00239573 -->

    <owl:NamedIndividual rdf:about="http://purl.obolibrary.org/obo/GAZ_00239573">
        <obo:IAO_0000115>A dam impounding Lake Gariep. Located between the Eastern Cape to the south and the Free State to the north and about 30 km north east of Colesberg. It is situated in a gorge at the entrance to the Ruigte Valley some 5 km east of Norvalspont. Completed 1971.</obo:IAO_0000115>
        <oboInOwl:hasOBONamespace>GAZ</oboInOwl:hasOBONamespace>
        <oboInOwl:id>GAZ:00239573</oboInOwl:id>
        <rdfs:label>Gariep Dam</rdfs:label>
    </owl:NamedIndividual>
    


    <!-- http://purl.obolibrary.org/obo/GAZ_00239574 -->

    <owl:NamedIndividual rdf:about="http://purl.obolibrary.org/obo/GAZ_00239574">
        <obo:RO_0001025 rdf:resource="http://purl.obolibrary.org/obo/GAZ_00002819"/>
        <obo:IAO_0000115>A protected area located approximately 12 km from Grahamstown off the N2 highway to Port Elizabeth.</obo:IAO_0000115>
        <oboInOwl:hasOBONamespace>GAZ</oboInOwl:hasOBONamespace>
        <oboInOwl:id>GAZ:00239574</oboInOwl:id>
        <rdfs:label>Thomas Baines Nature Reserve</rdfs:label>
    </owl:NamedIndividual>
    


    <!-- http://purl.obolibrary.org/obo/GAZ_00239575 -->

    <owl:NamedIndividual rdf:about="http://purl.obolibrary.org/obo/GAZ_00239575">
        <obo:RO_0001025 rdf:resource="http://purl.obolibrary.org/obo/GAZ_00076201"/>
        <obo:IAO_0000115>A protected area.</obo:IAO_0000115>
        <oboInOwl:hasOBONamespace>GAZ</oboInOwl:hasOBONamespace>
        <oboInOwl:id>GAZ:00239575</oboInOwl:id>
        <rdfs:label>Kouga Wilderness Area</rdfs:label>
    </owl:NamedIndividual>
    


    <!-- http://purl.obolibrary.org/obo/GAZ_00239576 -->

    <owl:NamedIndividual rdf:about="http://purl.obolibrary.org/obo/GAZ_00239576">
        <obo:RO_0001025 rdf:resource="http://purl.obolibrary.org/obo/GAZ_00076201"/>
        <obo:IAO_0000115>A protected area.</obo:IAO_0000115>
        <oboInOwl:hasOBONamespace>GAZ</oboInOwl:hasOBONamespace>
        <oboInOwl:id>GAZ:00239576</oboInOwl:id>
        <rdfs:label>Kouga Private Nature Reserve</rdfs:label>
    </owl:NamedIndividual>
    


    <!-- http://purl.obolibrary.org/obo/GAZ_00239577 -->

    <owl:NamedIndividual rdf:about="http://purl.obolibrary.org/obo/GAZ_00239577">
        <obo:RO_0001025 rdf:resource="http://purl.obolibrary.org/obo/GAZ_00076201"/>
        <obo:IAO_0000115>A protected area.</obo:IAO_0000115>
        <oboInOwl:hasOBONamespace>GAZ</oboInOwl:hasOBONamespace>
        <oboInOwl:id>GAZ:00239577</oboInOwl:id>
        <rdfs:label>Guerna Wilderness Area</rdfs:label>
    </owl:NamedIndividual>
    


    <!-- http://purl.obolibrary.org/obo/GAZ_00239578 -->

    <owl:NamedIndividual rdf:about="http://purl.obolibrary.org/obo/GAZ_00239578">
        <obo:RO_0001025 rdf:resource="http://purl.obolibrary.org/obo/GAZ_00076201"/>
        <obo:IAO_0000115>A protected area.</obo:IAO_0000115>
        <oboInOwl:hasOBONamespace>GAZ</oboInOwl:hasOBONamespace>
        <oboInOwl:id>GAZ:00239578</oboInOwl:id>
        <rdfs:label>Berg Plaatz Provincial Reserve</rdfs:label>
    </owl:NamedIndividual>
    


    <!-- http://purl.obolibrary.org/obo/GAZ_00239579 -->

    <owl:NamedIndividual rdf:about="http://purl.obolibrary.org/obo/GAZ_00239579">
        <obo:RO_0001025 rdf:resource="http://purl.obolibrary.org/obo/GAZ_00002813"/>
        <obo:IAO_0000115>A river.</obo:IAO_0000115>
        <oboInOwl:hasOBONamespace>GAZ</oboInOwl:hasOBONamespace>
        <oboInOwl:id>GAZ:00239579</oboInOwl:id>
        <rdfs:label>Nuwejaarspruit</rdfs:label>
    </owl:NamedIndividual>
    


    <!-- http://purl.obolibrary.org/obo/GAZ_00239580 -->

    <owl:NamedIndividual rdf:about="http://purl.obolibrary.org/obo/GAZ_00239580">
        <obo:RO_0001025 rdf:resource="http://purl.obolibrary.org/obo/GAZ_00239579"/>
        <obo:IAO_0000115>A dam. Located just outside the town of Harrismith, is part of the Tugela-Vaal Water Project. Impounds Sterkfontein Dam Reservoir. Completed 1977.</obo:IAO_0000115>
        <oboInOwl:hasOBONamespace>GAZ</oboInOwl:hasOBONamespace>
        <oboInOwl:id>GAZ:00239580</oboInOwl:id>
        <rdfs:label>Sterkfontein Dam</rdfs:label>
    </owl:NamedIndividual>
    


    <!-- http://purl.obolibrary.org/obo/GAZ_00239581 -->

    <owl:NamedIndividual rdf:about="http://purl.obolibrary.org/obo/GAZ_00239581">
        <obo:RO_0001025 rdf:resource="http://purl.obolibrary.org/obo/GAZ_00239579"/>
        <obo:IAO_0000115>A reservoir. Impounded by Sterkfontein Dam. Completed 1977.</obo:IAO_0000115>
        <oboInOwl:hasOBONamespace>GAZ</oboInOwl:hasOBONamespace>
        <oboInOwl:id>GAZ:00239581</oboInOwl:id>
        <rdfs:label>Sterkfontein Dam Reservoir</rdfs:label>
    </owl:NamedIndividual>
    


    <!-- http://purl.obolibrary.org/obo/GAZ_00239582 -->

    <owl:NamedIndividual rdf:about="http://purl.obolibrary.org/obo/GAZ_00239582">
        <obo:RO_0001025 rdf:resource="http://purl.obolibrary.org/obo/GAZ_00002812"/>
        <obo:IAO_0000115>The largest river in KwaZulu-Natal Province, South Africa. The river originates in the Drakensberg Mountains, Mont-aux-Sources. From the Drakensberg range the river meanders for 502 km through the KwaZulu-Natal midlands before discharging into the Indian Ocean.</obo:IAO_0000115>
        <oboInOwl:hasOBONamespace>GAZ</oboInOwl:hasOBONamespace>
        <oboInOwl:id>GAZ:00239582</oboInOwl:id>
        <rdfs:label>Tugela River</rdfs:label>
    </owl:NamedIndividual>
    


    <!-- http://purl.obolibrary.org/obo/GAZ_00239583 -->

    <owl:NamedIndividual rdf:about="http://purl.obolibrary.org/obo/GAZ_00239583">
        <obo:RO_0001025 rdf:resource="http://purl.obolibrary.org/obo/GAZ_00239582"/>
        <obo:IAO_0000115>A reservoir.</obo:IAO_0000115>
        <oboInOwl:hasOBONamespace>GAZ</oboInOwl:hasOBONamespace>
        <oboInOwl:id>GAZ:00239583</oboInOwl:id>
        <rdfs:label>Driel Barrage Dam</rdfs:label>
    </owl:NamedIndividual>
    


    <!-- http://purl.obolibrary.org/obo/GAZ_00239584 -->

    <owl:NamedIndividual rdf:about="http://purl.obolibrary.org/obo/GAZ_00239584">
        <obo:RO_0001025 rdf:resource="http://purl.obolibrary.org/obo/GAZ_00239582"/>
        <obo:IAO_0000115>A reservoir on the Tugela River in KwaZulu-Natal. Constructed 1973.</obo:IAO_0000115>
        <oboInOwl:hasOBONamespace>GAZ</oboInOwl:hasOBONamespace>
        <oboInOwl:id>GAZ:00239584</oboInOwl:id>
        <rdfs:label>Spioenkop Dam</rdfs:label>
    </owl:NamedIndividual>
    


    <!-- http://purl.obolibrary.org/obo/GAZ_00239585 -->

    <owl:NamedIndividual rdf:about="http://purl.obolibrary.org/obo/GAZ_00239585">
        <obo:RO_0001025 rdf:resource="http://purl.obolibrary.org/obo/GAZ_00239582"/>
        <obo:IAO_0000115>A dam. Constructed 1983.</obo:IAO_0000115>
        <oboInOwl:hasOBONamespace>GAZ</oboInOwl:hasOBONamespace>
        <oboInOwl:id>GAZ:00239585</oboInOwl:id>
        <rdfs:label>Woodstock Dam</rdfs:label>
    </owl:NamedIndividual>
    


    <!-- http://purl.obolibrary.org/obo/GAZ_00239588 -->

    <owl:NamedIndividual rdf:about="http://purl.obolibrary.org/obo/GAZ_00239588">
        <obo:RO_0001025 rdf:resource="http://purl.obolibrary.org/obo/GAZ_00002812"/>
        <obo:IAO_0000115>A river.</obo:IAO_0000115>
        <oboInOwl:hasOBONamespace>GAZ</oboInOwl:hasOBONamespace>
        <oboInOwl:id>GAZ:00239588</oboInOwl:id>
        <rdfs:label>Majaneni River</rdfs:label>
    </owl:NamedIndividual>
    


    <!-- http://purl.obolibrary.org/obo/GAZ_00239589 -->

    <owl:NamedIndividual rdf:about="http://purl.obolibrary.org/obo/GAZ_00239589">
        <obo:RO_0001025 rdf:resource="http://purl.obolibrary.org/obo/GAZ_00239588"/>
        <obo:IAO_0000115>A dam. Impounds Kilburn Dam Reservoir.</obo:IAO_0000115>
        <oboInOwl:hasOBONamespace>GAZ</oboInOwl:hasOBONamespace>
        <oboInOwl:id>GAZ:00239589</oboInOwl:id>
        <rdfs:label>Kilburn Dam</rdfs:label>
    </owl:NamedIndividual>
    


    <!-- http://purl.obolibrary.org/obo/GAZ_00239590 -->

    <owl:NamedIndividual rdf:about="http://purl.obolibrary.org/obo/GAZ_00239590">
        <obo:RO_0001025 rdf:resource="http://purl.obolibrary.org/obo/GAZ_00239588"/>
        <obo:IAO_0000115>A reservoir. Impounded by Kilburn Dam.</obo:IAO_0000115>
        <oboInOwl:hasOBONamespace>GAZ</oboInOwl:hasOBONamespace>
        <oboInOwl:id>GAZ:00239590</oboInOwl:id>
        <rdfs:label>Kilburn Dam Reservoir</rdfs:label>
    </owl:NamedIndividual>
    


    <!-- http://purl.obolibrary.org/obo/GAZ_00239591 -->

    <owl:NamedIndividual rdf:about="http://purl.obolibrary.org/obo/GAZ_00239591">
        <obo:IAO_0000115>A dam. Located on the Vaal River, downstream of Vaal Dam approximately 2 km upstream of the town of Bloemhof. Impounds Bloemhof Dam Reservoir. Completed 1970.</obo:IAO_0000115>
        <oboInOwl:hasOBONamespace>GAZ</oboInOwl:hasOBONamespace>
        <oboInOwl:id>GAZ:00239591</oboInOwl:id>
        <rdfs:label>Bloemhof Dam</rdfs:label>
    </owl:NamedIndividual>
    


    <!-- http://purl.obolibrary.org/obo/GAZ_00239592 -->

    <owl:NamedIndividual rdf:about="http://purl.obolibrary.org/obo/GAZ_00239592">
        <obo:IAO_0000115>A reservoir. Impounded by Bloemhof Dam. Completed 1970.</obo:IAO_0000115>
        <oboInOwl:hasOBONamespace>GAZ</oboInOwl:hasOBONamespace>
        <oboInOwl:id>GAZ:00239592</oboInOwl:id>
        <rdfs:label>Bloemhof Dam Reservoir</rdfs:label>
    </owl:NamedIndividual>
    


    <!-- http://purl.obolibrary.org/obo/GAZ_00239593 -->

    <owl:NamedIndividual rdf:about="http://purl.obolibrary.org/obo/GAZ_00239593">
        <obo:RO_0001025 rdf:resource="http://purl.obolibrary.org/obo/GAZ_00239595"/>
        <obo:IAO_0000115>A paleontological site. A series of fossil-bearing breccia filled cavities located almost exactly between the well known South African hominid-bearing sites of Sterkfontein and Kromdraai and about 40 km Northwest of the City of Johannesburg, South Africa.</obo:IAO_0000115>
        <oboInOwl:hasOBONamespace>GAZ</oboInOwl:hasOBONamespace>
        <oboInOwl:id>GAZ:00239593</oboInOwl:id>
        <rdfs:label>Coopers Cave Fossil Site</rdfs:label>
    </owl:NamedIndividual>
    


    <!-- http://purl.obolibrary.org/obo/GAZ_00239594 -->

    <owl:NamedIndividual rdf:about="http://purl.obolibrary.org/obo/GAZ_00239594">
        <obo:RO_0001025 rdf:resource="http://purl.obolibrary.org/obo/GAZ_00239595"/>
        <obo:IAO_0000115>A paleontologicial site. A fossil-bearing breccia filled cavity in South Africa. The cave is located about 4 km Southeast of the well known South African hominid-bearing sites of Sterkfontein and Kromdraai and about 36 km Northwest of the City of Johannesburg, South Africa.</obo:IAO_0000115>
        <oboInOwl:hasOBONamespace>GAZ</oboInOwl:hasOBONamespace>
        <oboInOwl:id>GAZ:00239594</oboInOwl:id>
        <rdfs:label>Plovers Lake Cave</rdfs:label>
    </owl:NamedIndividual>
    


    <!-- http://purl.obolibrary.org/obo/GAZ_00239595 -->

    <owl:NamedIndividual rdf:about="http://purl.obolibrary.org/obo/GAZ_00239595">
        <obo:RO_0001025 rdf:resource="http://purl.obolibrary.org/obo/GAZ_00002815"/>
        <obo:IAO_0000115>A paleontological site complex located about 50 km northwest of Johannesburg, South Africa in the Gauteng province. This site currently occupies 474 km2; it contains a complex of limestone caves. A World Heritage Site.</obo:IAO_0000115>
        <oboInOwl:hasOBONamespace>GAZ</oboInOwl:hasOBONamespace>
        <oboInOwl:id>GAZ:00239595</oboInOwl:id>
        <rdfs:label>Cradle of Humankind</rdfs:label>
    </owl:NamedIndividual>
    


    <!-- http://purl.obolibrary.org/obo/GAZ_00239596 -->

    <owl:NamedIndividual rdf:about="http://purl.obolibrary.org/obo/GAZ_00239596">
        <obo:RO_0001025 rdf:resource="http://purl.obolibrary.org/obo/GAZ_00239595"/>
        <obo:IAO_0000115>A paleontological site. A series of lime quarries some 2.5 km south-west of Sterkfontein Caves.</obo:IAO_0000115>
        <oboInOwl:hasOBONamespace>GAZ</oboInOwl:hasOBONamespace>
        <oboInOwl:id>GAZ:00239596</oboInOwl:id>
        <rdfs:label>Bolt&apos;s Farm</rdfs:label>
    </owl:NamedIndividual>
    


    <!-- http://purl.obolibrary.org/obo/GAZ_00239597 -->

    <owl:NamedIndividual rdf:about="http://purl.obolibrary.org/obo/GAZ_00239597">
        <obo:RO_0001025 rdf:resource="http://purl.obolibrary.org/obo/GAZ_00239595"/>
        <obo:IAO_0000115>A paleontological site located 1.6 km to the west of the Wonder Cave.</obo:IAO_0000115>
        <oboInOwl:hasOBONamespace>GAZ</oboInOwl:hasOBONamespace>
        <oboInOwl:id>GAZ:00239597</oboInOwl:id>
        <rdfs:label>Drimolen</rdfs:label>
    </owl:NamedIndividual>
    


    <!-- http://purl.obolibrary.org/obo/GAZ_00239598 -->

    <owl:NamedIndividual rdf:about="http://purl.obolibrary.org/obo/GAZ_00239598">
        <obo:RO_0001025 rdf:resource="http://purl.obolibrary.org/obo/GAZ_00002811"/>
        <obo:RO_0001025 rdf:resource="http://purl.obolibrary.org/obo/GAZ_00239595"/>
        <obo:IAO_0000115>A plaeontological site. Located 3.2 km south-west of Broederstroom village in North West Province.</obo:IAO_0000115>
        <oboInOwl:hasOBONamespace>GAZ</oboInOwl:hasOBONamespace>
        <oboInOwl:id>GAZ:00239598</oboInOwl:id>
        <rdfs:label>Gondolin</rdfs:label>
    </owl:NamedIndividual>
    


    <!-- http://purl.obolibrary.org/obo/GAZ_00239599 -->

    <owl:NamedIndividual rdf:about="http://purl.obolibrary.org/obo/GAZ_00239599">
        <obo:RO_0001025 rdf:resource="http://purl.obolibrary.org/obo/GAZ_00239595"/>
        <obo:IAO_0000115>A paleontological site.</obo:IAO_0000115>
        <oboInOwl:hasOBONamespace>GAZ</oboInOwl:hasOBONamespace>
        <oboInOwl:id>GAZ:00239599</oboInOwl:id>
        <rdfs:label>Haasgat</rdfs:label>
    </owl:NamedIndividual>
    


    <!-- http://purl.obolibrary.org/obo/GAZ_00239600 -->

    <owl:NamedIndividual rdf:about="http://purl.obolibrary.org/obo/GAZ_00239600">
        <obo:RO_0001025 rdf:resource="http://purl.obolibrary.org/obo/GAZ_00239595"/>
        <obo:IAO_0000115>A paleontological site. A fossil-bearing breccia filled cave located about 2 km east of the South African hominid-bearing site of Sterkfontein and about 45 km Northwest of the City of Johannesburg, South Africa.</obo:IAO_0000115>
        <oboInOwl:hasOBONamespace>GAZ</oboInOwl:hasOBONamespace>
        <oboInOwl:id>GAZ:00239600</oboInOwl:id>
        <rdfs:label>Kromdraai Fossil Site</rdfs:label>
    </owl:NamedIndividual>
    


    <!-- http://purl.obolibrary.org/obo/GAZ_00239601 -->

    <owl:NamedIndividual rdf:about="http://purl.obolibrary.org/obo/GAZ_00239601">
        <obo:RO_0001025 rdf:resource="http://purl.obolibrary.org/obo/GAZ_00239595"/>
        <obo:IAO_0000115>A paleontological site located about 1 .1 km to the north-west of the Kromdraai store on a steep hillside overlooking the BloubankspruIt.</obo:IAO_0000115>
        <oboInOwl:hasOBONamespace>GAZ</oboInOwl:hasOBONamespace>
        <oboInOwl:id>GAZ:00239601</oboInOwl:id>
        <rdfs:label>Minaars</rdfs:label>
    </owl:NamedIndividual>
    


    <!-- http://purl.obolibrary.org/obo/GAZ_00239602 -->

    <owl:NamedIndividual rdf:about="http://purl.obolibrary.org/obo/GAZ_00239602">
        <obo:RO_0001025 rdf:resource="http://purl.obolibrary.org/obo/GAZ_00239595"/>
        <obo:IAO_0000115>A paleontological site. A fossil-bearing breccia filled cavity located about 14 km East of the South African hominid-bearing sites of Sterkfontein and Kromdraai and about 45 km North-Northwest of the City of Johannesburg, South Africa.</obo:IAO_0000115>
        <oboInOwl:hasOBONamespace>GAZ</oboInOwl:hasOBONamespace>
        <oboInOwl:id>GAZ:00239602</oboInOwl:id>
        <rdfs:label>Motsetsi Cave</rdfs:label>
    </owl:NamedIndividual>
    


    <!-- http://purl.obolibrary.org/obo/GAZ_00239603 -->

    <owl:NamedIndividual rdf:about="http://purl.obolibrary.org/obo/GAZ_00239603">
        <obo:RO_0001025 rdf:resource="http://purl.obolibrary.org/obo/GAZ_00239595"/>
        <obo:IAO_0000115>A paleontological site. Limestone caves located within the Isaac Edwin Stegmann Reserve about 10 km from Krugersdorp.</obo:IAO_0000115>
        <oboInOwl:hasOBONamespace>GAZ</oboInOwl:hasOBONamespace>
        <oboInOwl:id>GAZ:00239603</oboInOwl:id>
        <rdfs:label>Sterkfontein Caves</rdfs:label>
    </owl:NamedIndividual>
    


    <!-- http://purl.obolibrary.org/obo/GAZ_00239604 -->

    <owl:NamedIndividual rdf:about="http://purl.obolibrary.org/obo/GAZ_00239604">
        <obo:RO_0001025 rdf:resource="http://purl.obolibrary.org/obo/GAZ_00239595"/>
        <obo:IAO_0000115>A paleontological site. Located about 1.5 km north-west of the Sterkfontein Caves.</obo:IAO_0000115>
        <oboInOwl:hasOBONamespace>GAZ</oboInOwl:hasOBONamespace>
        <oboInOwl:id>GAZ:00239604</oboInOwl:id>
        <rdfs:label>Swartkrans</rdfs:label>
    </owl:NamedIndividual>
    


    <!-- http://purl.obolibrary.org/obo/GAZ_00239605 -->

    <owl:NamedIndividual rdf:about="http://purl.obolibrary.org/obo/GAZ_00239605">
        <obo:RO_0001025 rdf:resource="http://purl.obolibrary.org/obo/GAZ_00076181"/>
        <obo:RO_0001025 rdf:resource="http://purl.obolibrary.org/obo/GAZ_00239595"/>
        <obo:IAO_0000115>A karst cave. Located in Kromdraai, Gauteng, South Africa.</obo:IAO_0000115>
        <oboInOwl:hasOBONamespace>GAZ</oboInOwl:hasOBONamespace>
        <oboInOwl:id>GAZ:00239605</oboInOwl:id>
        <rdfs:label>Wonder Cave</rdfs:label>
    </owl:NamedIndividual>
    


    <!-- http://purl.obolibrary.org/obo/GAZ_00239606 -->

    <owl:NamedIndividual rdf:about="http://purl.obolibrary.org/obo/GAZ_00239606">
        <obo:RO_0001025 rdf:resource="http://purl.obolibrary.org/obo/GAZ_00239595"/>
        <obo:IAO_0000115>A paleontological site. Three underground caves located 14 km north-east of Sterkfontein in the John Nash Nature Reserve.</obo:IAO_0000115>
        <oboInOwl:hasOBONamespace>GAZ</oboInOwl:hasOBONamespace>
        <oboInOwl:id>GAZ:00239606</oboInOwl:id>
        <rdfs:label>Gladysvale Cave</rdfs:label>
    </owl:NamedIndividual>
    


    <!-- http://purl.obolibrary.org/obo/GAZ_00239607 -->

    <owl:NamedIndividual rdf:about="http://purl.obolibrary.org/obo/GAZ_00239607">
        <obo:RO_0001025 rdf:resource="http://purl.obolibrary.org/obo/GAZ_00002815"/>
        <obo:IAO_0000115>A protected area.</obo:IAO_0000115>
        <oboInOwl:hasOBONamespace>GAZ</oboInOwl:hasOBONamespace>
        <oboInOwl:id>GAZ:00239607</oboInOwl:id>
        <rdfs:label>Krugersdorp Nature Reserve</rdfs:label>
    </owl:NamedIndividual>
    


    <!-- http://purl.obolibrary.org/obo/GAZ_00239608 -->

    <owl:NamedIndividual rdf:about="http://purl.obolibrary.org/obo/GAZ_00239608">
        <obo:RO_0001025 rdf:resource="http://purl.obolibrary.org/obo/GAZ_00005311"/>
        <obo:IAO_0000115>A protected area located in Pretoria.</obo:IAO_0000115>
        <oboInOwl:hasOBONamespace>GAZ</oboInOwl:hasOBONamespace>
        <oboInOwl:id>GAZ:00239608</oboInOwl:id>
        <rdfs:label>Rietvlei Nature Reserve</rdfs:label>
    </owl:NamedIndividual>
    


    <!-- http://purl.obolibrary.org/obo/GAZ_00239610 -->

    <owl:NamedIndividual rdf:about="http://purl.obolibrary.org/obo/GAZ_00239610">
        <obo:RO_0001025 rdf:resource="http://purl.obolibrary.org/obo/GAZ_00239608"/>
        <obo:IAO_0000115>A river.</obo:IAO_0000115>
        <oboInOwl:hasOBONamespace>GAZ</oboInOwl:hasOBONamespace>
        <oboInOwl:id>GAZ:00239610</oboInOwl:id>
        <rdfs:label>Rietvlei River</rdfs:label>
    </owl:NamedIndividual>
    


    <!-- http://purl.obolibrary.org/obo/GAZ_00239611 -->

    <owl:NamedIndividual rdf:about="http://purl.obolibrary.org/obo/GAZ_00239611">
        <obo:RO_0001025 rdf:resource="http://purl.obolibrary.org/obo/GAZ_00239610"/>
        <obo:IAO_0000115>A dam. Constructed 1932-1934.</obo:IAO_0000115>
        <oboInOwl:hasOBONamespace>GAZ</oboInOwl:hasOBONamespace>
        <oboInOwl:id>GAZ:00239611</oboInOwl:id>
        <rdfs:label>Rietvlei Dam</rdfs:label>
    </owl:NamedIndividual>
    


    <!-- http://purl.obolibrary.org/obo/GAZ_00239612 -->

    <owl:NamedIndividual rdf:about="http://purl.obolibrary.org/obo/GAZ_00239612">
        <obo:RO_0001025 rdf:resource="http://purl.obolibrary.org/obo/GAZ_00002815"/>
        <obo:IAO_0000115>A river in Gauteng Province, South Africa.</obo:IAO_0000115>
        <oboInOwl:hasOBONamespace>GAZ</oboInOwl:hasOBONamespace>
        <oboInOwl:id>GAZ:00239612</oboInOwl:id>
        <rdfs:label>Hennops River</rdfs:label>
    </owl:NamedIndividual>
    


    <!-- http://purl.obolibrary.org/obo/GAZ_00239613 -->

    <owl:NamedIndividual rdf:about="http://purl.obolibrary.org/obo/GAZ_00239613">
        <obo:RO_0001025 rdf:resource="http://purl.obolibrary.org/obo/GAZ_00002815"/>
        <obo:IAO_0000115>A protected area located S of Suikerbosrand Nature Reserve.</obo:IAO_0000115>
        <oboInOwl:hasOBONamespace>GAZ</oboInOwl:hasOBONamespace>
        <oboInOwl:id>GAZ:00239613</oboInOwl:id>
        <rdfs:label>Alice Glockner Nature Reserve</rdfs:label>
    </owl:NamedIndividual>
    


    <!-- http://purl.obolibrary.org/obo/GAZ_00239616 -->

    <owl:NamedIndividual rdf:about="http://purl.obolibrary.org/obo/GAZ_00239616">
        <obo:IAO_0000115>A dam. Impounds Roodeplaat Dam Reservoir. Constructed 1955-1959.</obo:IAO_0000115>
        <oboInOwl:hasOBONamespace>GAZ</oboInOwl:hasOBONamespace>
        <oboInOwl:id>GAZ:00239616</oboInOwl:id>
        <rdfs:label>Roodeplaat Dam</rdfs:label>
    </owl:NamedIndividual>
    


    <!-- http://purl.obolibrary.org/obo/GAZ_00239617 -->

    <owl:NamedIndividual rdf:about="http://purl.obolibrary.org/obo/GAZ_00239617">
        <obo:IAO_0000115>A reservoir. Impounded by Roodeplaat Dam. Constructed 1955-1959.</obo:IAO_0000115>
        <oboInOwl:hasOBONamespace>GAZ</oboInOwl:hasOBONamespace>
        <oboInOwl:id>GAZ:00239617</oboInOwl:id>
        <rdfs:label>Roodeplaat Dam Reservoir</rdfs:label>
    </owl:NamedIndividual>
    


    <!-- http://purl.obolibrary.org/obo/GAZ_00239618 -->

    <owl:NamedIndividual rdf:about="http://purl.obolibrary.org/obo/GAZ_00239618">
        <obo:RO_0001025 rdf:resource="http://purl.obolibrary.org/obo/GAZ_00003035"/>
        <obo:IAO_0000115>An administrative region of Johannesburg.</obo:IAO_0000115>
        <oboInOwl:hasOBONamespace>GAZ</oboInOwl:hasOBONamespace>
        <oboInOwl:id>GAZ:00239618</oboInOwl:id>
        <rdfs:label>Region A</rdfs:label>
    </owl:NamedIndividual>
    


    <!-- http://purl.obolibrary.org/obo/GAZ_00239619 -->

    <owl:NamedIndividual rdf:about="http://purl.obolibrary.org/obo/GAZ_00239619">
        <obo:RO_0001025 rdf:resource="http://purl.obolibrary.org/obo/GAZ_00003035"/>
        <obo:IAO_0000115>An administrative region of Johannesburg.</obo:IAO_0000115>
        <oboInOwl:hasOBONamespace>GAZ</oboInOwl:hasOBONamespace>
        <oboInOwl:id>GAZ:00239619</oboInOwl:id>
        <rdfs:label>Region B</rdfs:label>
    </owl:NamedIndividual>
    


    <!-- http://purl.obolibrary.org/obo/GAZ_00239620 -->

    <owl:NamedIndividual rdf:about="http://purl.obolibrary.org/obo/GAZ_00239620">
        <obo:RO_0001025 rdf:resource="http://purl.obolibrary.org/obo/GAZ_00003035"/>
        <obo:IAO_0000115>An administrative region of Johannesburg.</obo:IAO_0000115>
        <oboInOwl:hasOBONamespace>GAZ</oboInOwl:hasOBONamespace>
        <oboInOwl:id>GAZ:00239620</oboInOwl:id>
        <rdfs:label>Region C</rdfs:label>
    </owl:NamedIndividual>
    


    <!-- http://purl.obolibrary.org/obo/GAZ_00239621 -->

    <owl:NamedIndividual rdf:about="http://purl.obolibrary.org/obo/GAZ_00239621">
        <obo:RO_0001025 rdf:resource="http://purl.obolibrary.org/obo/GAZ_00003035"/>
        <obo:IAO_0000115>An administrative region of Johannesburg.</obo:IAO_0000115>
        <oboInOwl:hasOBONamespace>GAZ</oboInOwl:hasOBONamespace>
        <oboInOwl:id>GAZ:00239621</oboInOwl:id>
        <rdfs:label>Region D</rdfs:label>
    </owl:NamedIndividual>
    


    <!-- http://purl.obolibrary.org/obo/GAZ_00239622 -->

    <owl:NamedIndividual rdf:about="http://purl.obolibrary.org/obo/GAZ_00239622">
        <obo:RO_0001025 rdf:resource="http://purl.obolibrary.org/obo/GAZ_00003035"/>
        <obo:IAO_0000115>An administrative region of Johannesburg.</obo:IAO_0000115>
        <oboInOwl:hasOBONamespace>GAZ</oboInOwl:hasOBONamespace>
        <oboInOwl:id>GAZ:00239622</oboInOwl:id>
        <rdfs:label>Region E</rdfs:label>
    </owl:NamedIndividual>
    


    <!-- http://purl.obolibrary.org/obo/GAZ_00239623 -->

    <owl:NamedIndividual rdf:about="http://purl.obolibrary.org/obo/GAZ_00239623">
        <obo:RO_0001025 rdf:resource="http://purl.obolibrary.org/obo/GAZ_00003035"/>
        <obo:IAO_0000115>An administrative region of Johannesburg.</obo:IAO_0000115>
        <oboInOwl:hasOBONamespace>GAZ</oboInOwl:hasOBONamespace>
        <oboInOwl:id>GAZ:00239623</oboInOwl:id>
        <rdfs:label>Region F</rdfs:label>
    </owl:NamedIndividual>
    


    <!-- http://purl.obolibrary.org/obo/GAZ_00239624 -->

    <owl:NamedIndividual rdf:about="http://purl.obolibrary.org/obo/GAZ_00239624">
        <obo:RO_0001025 rdf:resource="http://purl.obolibrary.org/obo/GAZ_00003035"/>
        <obo:IAO_0000115>An administrative region of Johannesburg.</obo:IAO_0000115>
        <oboInOwl:hasOBONamespace>GAZ</oboInOwl:hasOBONamespace>
        <oboInOwl:id>GAZ:00239624</oboInOwl:id>
        <rdfs:label>Region G</rdfs:label>
    </owl:NamedIndividual>
    


    <!-- http://purl.obolibrary.org/obo/GAZ_00239625 -->

    <owl:NamedIndividual rdf:about="http://purl.obolibrary.org/obo/GAZ_00239625">
        <rdf:type rdf:resource="http://purl.obolibrary.org/obo/ENVO_00000856"/>
        <obo:RO_0001025 rdf:resource="http://purl.obolibrary.org/obo/GAZ_00239621"/>
        <obo:IAO_0000115>An urban area of the City of Johannesburg in Gauteng, South Africa, bordering the city&apos;s mining belt in the north.</obo:IAO_0000115>
        <oboInOwl:hasOBONamespace>GAZ</oboInOwl:hasOBONamespace>
        <oboInOwl:id>GAZ:00239625</oboInOwl:id>
        <rdfs:label>Soweto</rdfs:label>
    </owl:NamedIndividual>
    


    <!-- http://purl.obolibrary.org/obo/GAZ_00239626 -->

    <owl:NamedIndividual rdf:about="http://purl.obolibrary.org/obo/GAZ_00239626">
        <rdf:type rdf:resource="http://purl.obolibrary.org/obo/ENVO_00000856"/>
        <obo:RO_0001025 rdf:resource="http://purl.obolibrary.org/obo/GAZ_00075922"/>
        <obo:IAO_0000115>A populated place. A town.</obo:IAO_0000115>
        <oboInOwl:hasOBONamespace>GAZ</oboInOwl:hasOBONamespace>
        <oboInOwl:id>GAZ:00239626</oboInOwl:id>
        <rdfs:label>Eshowe</rdfs:label>
    </owl:NamedIndividual>
    


    <!-- http://purl.obolibrary.org/obo/GAZ_00239627 -->

    <owl:NamedIndividual rdf:about="http://purl.obolibrary.org/obo/GAZ_00239627">
        <obo:RO_0001025 rdf:resource="http://purl.obolibrary.org/obo/GAZ_00239626"/>
        <obo:IAO_0000115>A subtropical forest in Eshowe, Zululand, South Africa.</obo:IAO_0000115>
        <oboInOwl:hasOBONamespace>GAZ</oboInOwl:hasOBONamespace>
        <oboInOwl:id>GAZ:00239627</oboInOwl:id>
        <rdfs:label>Dhlinza Forest</rdfs:label>
    </owl:NamedIndividual>
    


    <!-- http://purl.obolibrary.org/obo/GAZ_00239628 -->

    <owl:NamedIndividual rdf:about="http://purl.obolibrary.org/obo/GAZ_00239628">
        <obo:RO_0001025 rdf:resource="http://purl.obolibrary.org/obo/GAZ_00002812"/>
        <obo:IAO_0000115>A river in KwaZulu-Natal, a province of South Africa. It is formed by the confluence of the Black (Imfolozi emnyama) and White Umfolozi (Imfolozi emhlope) Rivers near the southeastern boundary of the Hluhluwe-Umfolozi Game Reserve. The river flows in an easterly direction to the Indian Ocean at Maphelana.</obo:IAO_0000115>
        <oboInOwl:hasOBONamespace>GAZ</oboInOwl:hasOBONamespace>
        <oboInOwl:id>GAZ:00239628</oboInOwl:id>
        <rdfs:label>Umfolozi River</rdfs:label>
    </owl:NamedIndividual>
    


    <!-- http://purl.obolibrary.org/obo/GAZ_00239631 -->

    <owl:NamedIndividual rdf:about="http://purl.obolibrary.org/obo/GAZ_00239631">
        <obo:RO_0001025 rdf:resource="http://purl.obolibrary.org/obo/GAZ_00011816"/>
        <obo:IAO_0000115>A dam. Impounds Midmar Dam Reservoir.</obo:IAO_0000115>
        <oboInOwl:hasOBONamespace>GAZ</oboInOwl:hasOBONamespace>
        <oboInOwl:id>GAZ:00239631</oboInOwl:id>
        <rdfs:label>Midmar Dam</rdfs:label>
    </owl:NamedIndividual>
    


    <!-- http://purl.obolibrary.org/obo/GAZ_00239632 -->

    <owl:NamedIndividual rdf:about="http://purl.obolibrary.org/obo/GAZ_00239632">
        <obo:RO_0001025 rdf:resource="http://purl.obolibrary.org/obo/GAZ_00011816"/>
        <obo:IAO_0000115>A dam.</obo:IAO_0000115>
        <oboInOwl:hasOBONamespace>GAZ</oboInOwl:hasOBONamespace>
        <oboInOwl:id>GAZ:00239632</oboInOwl:id>
        <rdfs:label>Albert Falls Dam</rdfs:label>
    </owl:NamedIndividual>
    


    <!-- http://purl.obolibrary.org/obo/GAZ_00239633 -->

    <owl:NamedIndividual rdf:about="http://purl.obolibrary.org/obo/GAZ_00239633">
        <obo:RO_0001025 rdf:resource="http://purl.obolibrary.org/obo/GAZ_00011816"/>
        <obo:IAO_0000115>A dam.</obo:IAO_0000115>
        <oboInOwl:hasOBONamespace>GAZ</oboInOwl:hasOBONamespace>
        <oboInOwl:id>GAZ:00239633</oboInOwl:id>
        <rdfs:label>Nagle Dam</rdfs:label>
    </owl:NamedIndividual>
    


    <!-- http://purl.obolibrary.org/obo/GAZ_00239634 -->

    <owl:NamedIndividual rdf:about="http://purl.obolibrary.org/obo/GAZ_00239634">
        <obo:RO_0001025 rdf:resource="http://purl.obolibrary.org/obo/GAZ_00011816"/>
        <oboInOwl:hasOBONamespace>GAZ</oboInOwl:hasOBONamespace>
        <oboInOwl:id>GAZ:00239634</oboInOwl:id>
        <rdfs:label>Inanda Dam</rdfs:label>
    </owl:NamedIndividual>
    


    <!-- http://purl.obolibrary.org/obo/GAZ_00239635 -->

    <owl:NamedIndividual rdf:about="http://purl.obolibrary.org/obo/GAZ_00239635">
        <obo:RO_0001025 rdf:resource="http://purl.obolibrary.org/obo/GAZ_00011816"/>
        <obo:IAO_0000115>A reservoir. Impounded by Midmar Dam.</obo:IAO_0000115>
        <oboInOwl:hasOBONamespace>GAZ</oboInOwl:hasOBONamespace>
        <oboInOwl:id>GAZ:00239635</oboInOwl:id>
        <rdfs:label>Midmar Dam Reservoir</rdfs:label>
    </owl:NamedIndividual>
    


    <!-- http://purl.obolibrary.org/obo/GAZ_00239636 -->

    <owl:NamedIndividual rdf:about="http://purl.obolibrary.org/obo/GAZ_00239636">
        <obo:RO_0001025 rdf:resource="http://purl.obolibrary.org/obo/GAZ_00002812"/>
        <obo:IAO_0000115>A river. A tributary of the Mngeni River.</obo:IAO_0000115>
        <oboInOwl:hasOBONamespace>GAZ</oboInOwl:hasOBONamespace>
        <oboInOwl:id>GAZ:00239636</oboInOwl:id>
        <rdfs:label>Msunduzi River</rdfs:label>
    </owl:NamedIndividual>
    


    <!-- http://purl.obolibrary.org/obo/GAZ_00239637 -->

    <owl:NamedIndividual rdf:about="http://purl.obolibrary.org/obo/GAZ_00239637">
        <obo:RO_0001025 rdf:resource="http://purl.obolibrary.org/obo/GAZ_00076208"/>
        <obo:IAO_0000115>A canyon located along the spectacular forest-cloaked ravine of the Mzimkulwana river just west of Port Shepstone.</obo:IAO_0000115>
        <oboInOwl:hasOBONamespace>GAZ</oboInOwl:hasOBONamespace>
        <oboInOwl:id>GAZ:00239637</oboInOwl:id>
        <rdfs:label>Oribi Gorge</rdfs:label>
    </owl:NamedIndividual>
    


    <!-- http://purl.obolibrary.org/obo/GAZ_00239638 -->

    <owl:NamedIndividual rdf:about="http://purl.obolibrary.org/obo/GAZ_00239638">
        <obo:RO_0001025 rdf:resource="http://purl.obolibrary.org/obo/GAZ_00239637"/>
        <obo:IAO_0000115>A river.</obo:IAO_0000115>
        <oboInOwl:hasOBONamespace>GAZ</oboInOwl:hasOBONamespace>
        <oboInOwl:id>GAZ:00239638</oboInOwl:id>
        <rdfs:label>Mzimkulwana River</rdfs:label>
    </owl:NamedIndividual>
    


    <!-- http://purl.obolibrary.org/obo/GAZ_00239639 -->

    <owl:NamedIndividual rdf:about="http://purl.obolibrary.org/obo/GAZ_00239639">
        <rdf:type rdf:resource="http://purl.obolibrary.org/obo/ENVO_00000856"/>
        <obo:RO_0001025 rdf:resource="http://purl.obolibrary.org/obo/GAZ_00075897"/>
        <obo:IAO_0000115>A populated place. A town located at the mouth of the Mzimkulu River.</obo:IAO_0000115>
        <oboInOwl:hasOBONamespace>GAZ</oboInOwl:hasOBONamespace>
        <oboInOwl:id>GAZ:00239639</oboInOwl:id>
        <rdfs:label>Port Shepstone</rdfs:label>
    </owl:NamedIndividual>
    


    <!-- http://purl.obolibrary.org/obo/GAZ_00239641 -->

    <owl:NamedIndividual rdf:about="http://purl.obolibrary.org/obo/GAZ_00239641">
        <obo:RO_0001025 rdf:resource="http://purl.obolibrary.org/obo/GAZ_00012787"/>
        <obo:IAO_0000115>A populated place. An administrative town in a dairy and cattle farming community in the Mzimkulu River valley of KwaZulu-Natal, South Africa.</obo:IAO_0000115>
        <oboInOwl:hasOBONamespace>GAZ</oboInOwl:hasOBONamespace>
        <oboInOwl:id>GAZ:00239641</oboInOwl:id>
        <rdfs:label>Underberg</rdfs:label>
    </owl:NamedIndividual>
    


    <!-- http://purl.obolibrary.org/obo/GAZ_00239642 -->

    <owl:NamedIndividual rdf:about="http://purl.obolibrary.org/obo/GAZ_00239642">
        <obo:IAO_0000115>A dam.</obo:IAO_0000115>
        <oboInOwl:hasOBONamespace>GAZ</oboInOwl:hasOBONamespace>
        <oboInOwl:id>GAZ:00239642</oboInOwl:id>
        <rdfs:label>Pongolapoort Dam</rdfs:label>
    </owl:NamedIndividual>
    


    <!-- http://purl.obolibrary.org/obo/GAZ_00239644 -->

    <owl:NamedIndividual rdf:about="http://purl.obolibrary.org/obo/GAZ_00239644">
        <obo:RO_0001025 rdf:resource="http://purl.obolibrary.org/obo/GAZ_00239785"/>
        <obo:IAO_0000115>A protected area located in the KwaZulu Natal province of South Africa and forms part of the uKhahlamba Drakensberg Park World Heritage Site.</obo:IAO_0000115>
        <oboInOwl:hasOBONamespace>GAZ</oboInOwl:hasOBONamespace>
        <oboInOwl:id>GAZ:00239644</oboInOwl:id>
        <rdfs:label>Royal Natal National Park</rdfs:label>
    </owl:NamedIndividual>
    


    <!-- http://purl.obolibrary.org/obo/GAZ_00239645 -->

    <owl:NamedIndividual rdf:about="http://purl.obolibrary.org/obo/GAZ_00239645">
        <obo:RO_0001025 rdf:resource="http://purl.obolibrary.org/obo/GAZ_00005308"/>
        <obo:IAO_0000115>A bay.</obo:IAO_0000115>
        <oboInOwl:hasOBONamespace>GAZ</oboInOwl:hasOBONamespace>
        <oboInOwl:id>GAZ:00239645</oboInOwl:id>
        <rdfs:label>Sodwana Bay</rdfs:label>
    </owl:NamedIndividual>
    


    <!-- http://purl.obolibrary.org/obo/GAZ_00239646 -->

    <owl:NamedIndividual rdf:about="http://purl.obolibrary.org/obo/GAZ_00239646">
        <obo:RO_0001025 rdf:resource="http://purl.obolibrary.org/obo/GAZ_00002812"/>
        <obo:IAO_0000115>A protected area located on the Indian Ocean coastline in Northern KwaZulu-Natal between the Tugela and Amatikulu River mouths.</obo:IAO_0000115>
        <oboInOwl:hasOBONamespace>GAZ</oboInOwl:hasOBONamespace>
        <oboInOwl:id>GAZ:00239646</oboInOwl:id>
        <rdfs:label>Amatikulu Nature Reserve</rdfs:label>
    </owl:NamedIndividual>
    


    <!-- http://purl.obolibrary.org/obo/GAZ_00239647 -->

    <owl:NamedIndividual rdf:about="http://purl.obolibrary.org/obo/GAZ_00239647">
        <obo:RO_0001025 rdf:resource="http://purl.obolibrary.org/obo/GAZ_00010007"/>
        <oboInOwl:hasOBONamespace>GAZ</oboInOwl:hasOBONamespace>
        <oboInOwl:id>GAZ:00239647</oboInOwl:id>
        <rdfs:label>North Central Region</rdfs:label>
    </owl:NamedIndividual>
    


    <!-- http://purl.obolibrary.org/obo/GAZ_00239648 -->

    <owl:NamedIndividual rdf:about="http://purl.obolibrary.org/obo/GAZ_00239648">
        <obo:RO_0001025 rdf:resource="http://purl.obolibrary.org/obo/GAZ_00010007"/>
        <oboInOwl:hasOBONamespace>GAZ</oboInOwl:hasOBONamespace>
        <oboInOwl:id>GAZ:00239648</oboInOwl:id>
        <rdfs:label>South Central Region</rdfs:label>
    </owl:NamedIndividual>
    


    <!-- http://purl.obolibrary.org/obo/GAZ_00239649 -->

    <owl:NamedIndividual rdf:about="http://purl.obolibrary.org/obo/GAZ_00239649">
        <obo:RO_0001025 rdf:resource="http://purl.obolibrary.org/obo/GAZ_00010007"/>
        <oboInOwl:hasOBONamespace>GAZ</oboInOwl:hasOBONamespace>
        <oboInOwl:id>GAZ:00239649</oboInOwl:id>
        <rdfs:label>North Region</rdfs:label>
    </owl:NamedIndividual>
    


    <!-- http://purl.obolibrary.org/obo/GAZ_00239650 -->

    <owl:NamedIndividual rdf:about="http://purl.obolibrary.org/obo/GAZ_00239650">
        <obo:RO_0001025 rdf:resource="http://purl.obolibrary.org/obo/GAZ_00010007"/>
        <oboInOwl:hasOBONamespace>GAZ</oboInOwl:hasOBONamespace>
        <oboInOwl:id>GAZ:00239650</oboInOwl:id>
        <rdfs:label>Outer West Region</rdfs:label>
    </owl:NamedIndividual>
    


    <!-- http://purl.obolibrary.org/obo/GAZ_00239651 -->

    <owl:NamedIndividual rdf:about="http://purl.obolibrary.org/obo/GAZ_00239651">
        <obo:RO_0001025 rdf:resource="http://purl.obolibrary.org/obo/GAZ_00010007"/>
        <oboInOwl:hasOBONamespace>GAZ</oboInOwl:hasOBONamespace>
        <oboInOwl:id>GAZ:00239651</oboInOwl:id>
        <rdfs:label>Inner West Region</rdfs:label>
    </owl:NamedIndividual>
    


    <!-- http://purl.obolibrary.org/obo/GAZ_00239652 -->

    <owl:NamedIndividual rdf:about="http://purl.obolibrary.org/obo/GAZ_00239652">
        <obo:RO_0001025 rdf:resource="http://purl.obolibrary.org/obo/GAZ_00010007"/>
        <oboInOwl:hasOBONamespace>GAZ</oboInOwl:hasOBONamespace>
        <oboInOwl:id>GAZ:00239652</oboInOwl:id>
        <rdfs:label>South Region</rdfs:label>
    </owl:NamedIndividual>
    


    <!-- http://purl.obolibrary.org/obo/GAZ_00239653 -->

    <owl:NamedIndividual rdf:about="http://purl.obolibrary.org/obo/GAZ_00239653">
        <obo:RO_0001025 rdf:resource="http://purl.obolibrary.org/obo/GAZ_00239647"/>
        <obo:IAO_0000115>A suburb of Durban.</obo:IAO_0000115>
        <oboInOwl:hasOBONamespace>GAZ</oboInOwl:hasOBONamespace>
        <oboInOwl:id>GAZ:00239653</oboInOwl:id>
        <rdfs:label>Asherville</rdfs:label>
    </owl:NamedIndividual>
    


    <!-- http://purl.obolibrary.org/obo/GAZ_00239654 -->

    <owl:NamedIndividual rdf:about="http://purl.obolibrary.org/obo/GAZ_00239654">
        <obo:RO_0001025 rdf:resource="http://purl.obolibrary.org/obo/GAZ_00239647"/>
        <obo:IAO_0000115>A suburb of Durban.</obo:IAO_0000115>
        <oboInOwl:hasOBONamespace>GAZ</oboInOwl:hasOBONamespace>
        <oboInOwl:id>GAZ:00239654</oboInOwl:id>
        <rdfs:label>Berea</rdfs:label>
    </owl:NamedIndividual>
    


    <!-- http://purl.obolibrary.org/obo/GAZ_00239655 -->

    <owl:NamedIndividual rdf:about="http://purl.obolibrary.org/obo/GAZ_00239655">
        <obo:RO_0001025 rdf:resource="http://purl.obolibrary.org/obo/GAZ_00239647"/>
        <obo:IAO_0000115>A suburb of Durban.</obo:IAO_0000115>
        <oboInOwl:hasOBONamespace>GAZ</oboInOwl:hasOBONamespace>
        <oboInOwl:id>GAZ:00239655</oboInOwl:id>
        <rdfs:label>Bluff</rdfs:label>
    </owl:NamedIndividual>
    


    <!-- http://purl.obolibrary.org/obo/GAZ_00239656 -->

    <owl:NamedIndividual rdf:about="http://purl.obolibrary.org/obo/GAZ_00239656">
        <obo:RO_0001025 rdf:resource="http://purl.obolibrary.org/obo/GAZ_00239647"/>
        <obo:IAO_0000115>A suburb of Durban.</obo:IAO_0000115>
        <oboInOwl:hasOBONamespace>GAZ</oboInOwl:hasOBONamespace>
        <oboInOwl:id>GAZ:00239656</oboInOwl:id>
        <rdfs:label>Clare Estate</rdfs:label>
    </owl:NamedIndividual>
    


    <!-- http://purl.obolibrary.org/obo/GAZ_00239657 -->

    <owl:NamedIndividual rdf:about="http://purl.obolibrary.org/obo/GAZ_00239657">
        <obo:RO_0001025 rdf:resource="http://purl.obolibrary.org/obo/GAZ_00239647"/>
        <obo:IAO_0000115>A suburb of Durban.</obo:IAO_0000115>
        <oboInOwl:hasOBONamespace>GAZ</oboInOwl:hasOBONamespace>
        <oboInOwl:id>GAZ:00239657</oboInOwl:id>
        <rdfs:label>Durban North</rdfs:label>
    </owl:NamedIndividual>
    


    <!-- http://purl.obolibrary.org/obo/GAZ_00239658 -->

    <owl:NamedIndividual rdf:about="http://purl.obolibrary.org/obo/GAZ_00239658">
        <obo:RO_0001025 rdf:resource="http://purl.obolibrary.org/obo/GAZ_00239647"/>
        <obo:IAO_0000115>A suburb of Durban.</obo:IAO_0000115>
        <oboInOwl:hasOBONamespace>GAZ</oboInOwl:hasOBONamespace>
        <oboInOwl:id>GAZ:00239658</oboInOwl:id>
        <rdfs:label>Duff&apos;s Road</rdfs:label>
    </owl:NamedIndividual>
    


    <!-- http://purl.obolibrary.org/obo/GAZ_00239659 -->

    <owl:NamedIndividual rdf:about="http://purl.obolibrary.org/obo/GAZ_00239659">
        <obo:RO_0001025 rdf:resource="http://purl.obolibrary.org/obo/GAZ_00239647"/>
        <obo:IAO_0000115>A suburb of Durban.</obo:IAO_0000115>
        <oboInOwl:hasOBONamespace>GAZ</oboInOwl:hasOBONamespace>
        <oboInOwl:id>GAZ:00239659</oboInOwl:id>
        <rdfs:label>Greyville</rdfs:label>
    </owl:NamedIndividual>
    


    <!-- http://purl.obolibrary.org/obo/GAZ_00239660 -->

    <owl:NamedIndividual rdf:about="http://purl.obolibrary.org/obo/GAZ_00239660">
        <obo:RO_0001025 rdf:resource="http://purl.obolibrary.org/obo/GAZ_00239647"/>
        <obo:IAO_0000115>A suburb of Durban.</obo:IAO_0000115>
        <oboInOwl:hasOBONamespace>GAZ</oboInOwl:hasOBONamespace>
        <oboInOwl:id>GAZ:00239660</oboInOwl:id>
        <rdfs:label>Inanda-Glebe</rdfs:label>
    </owl:NamedIndividual>
    


    <!-- http://purl.obolibrary.org/obo/GAZ_00239661 -->

    <owl:NamedIndividual rdf:about="http://purl.obolibrary.org/obo/GAZ_00239661">
        <obo:RO_0001025 rdf:resource="http://purl.obolibrary.org/obo/GAZ_00239647"/>
        <obo:IAO_0000115>A suburb of Durban.</obo:IAO_0000115>
        <oboInOwl:hasOBONamespace>GAZ</oboInOwl:hasOBONamespace>
        <oboInOwl:id>GAZ:00239661</oboInOwl:id>
        <rdfs:label>Inanda-Newtown</rdfs:label>
    </owl:NamedIndividual>
    


    <!-- http://purl.obolibrary.org/obo/GAZ_00239662 -->

    <owl:NamedIndividual rdf:about="http://purl.obolibrary.org/obo/GAZ_00239662">
        <obo:RO_0001025 rdf:resource="http://purl.obolibrary.org/obo/GAZ_00239647"/>
        <obo:IAO_0000115>A suburb of Durban.</obo:IAO_0000115>
        <oboInOwl:hasOBONamespace>GAZ</oboInOwl:hasOBONamespace>
        <oboInOwl:id>GAZ:00239662</oboInOwl:id>
        <rdfs:label>KwaDinabukubo</rdfs:label>
    </owl:NamedIndividual>
    


    <!-- http://purl.obolibrary.org/obo/GAZ_00239663 -->

    <owl:NamedIndividual rdf:about="http://purl.obolibrary.org/obo/GAZ_00239663">
        <obo:RO_0001025 rdf:resource="http://purl.obolibrary.org/obo/GAZ_00239647"/>
        <obo:IAO_0000115>A suburb of Durban.</obo:IAO_0000115>
        <oboInOwl:hasOBONamespace>GAZ</oboInOwl:hasOBONamespace>
        <oboInOwl:id>GAZ:00239663</oboInOwl:id>
        <rdfs:label>KwaMashu</rdfs:label>
    </owl:NamedIndividual>
    


    <!-- http://purl.obolibrary.org/obo/GAZ_00239664 -->

    <owl:NamedIndividual rdf:about="http://purl.obolibrary.org/obo/GAZ_00239664">
        <obo:RO_0001025 rdf:resource="http://purl.obolibrary.org/obo/GAZ_00239647"/>
        <obo:IAO_0000115>A suburb of Durban.</obo:IAO_0000115>
        <oboInOwl:hasOBONamespace>GAZ</oboInOwl:hasOBONamespace>
        <oboInOwl:id>GAZ:00239664</oboInOwl:id>
        <rdfs:label>Mayville</rdfs:label>
    </owl:NamedIndividual>
    


    <!-- http://purl.obolibrary.org/obo/GAZ_00239665 -->

    <owl:NamedIndividual rdf:about="http://purl.obolibrary.org/obo/GAZ_00239665">
        <obo:RO_0001025 rdf:resource="http://purl.obolibrary.org/obo/GAZ_00239647"/>
        <obo:IAO_0000115>A suburb of Durban.</obo:IAO_0000115>
        <oboInOwl:hasOBONamespace>GAZ</oboInOwl:hasOBONamespace>
        <oboInOwl:id>GAZ:00239665</oboInOwl:id>
        <rdfs:label>Morningside</rdfs:label>
    </owl:NamedIndividual>
    


    <!-- http://purl.obolibrary.org/obo/GAZ_00239666 -->

    <owl:NamedIndividual rdf:about="http://purl.obolibrary.org/obo/GAZ_00239666">
        <obo:RO_0001025 rdf:resource="http://purl.obolibrary.org/obo/GAZ_00239647"/>
        <obo:IAO_0000115>A suburb of Durban.</obo:IAO_0000115>
        <oboInOwl:hasOBONamespace>GAZ</oboInOwl:hasOBONamespace>
        <oboInOwl:id>GAZ:00239666</oboInOwl:id>
        <rdfs:label>Ntuzuma</rdfs:label>
    </owl:NamedIndividual>
    


    <!-- http://purl.obolibrary.org/obo/GAZ_00239667 -->

    <owl:NamedIndividual rdf:about="http://purl.obolibrary.org/obo/GAZ_00239667">
        <obo:RO_0001025 rdf:resource="http://purl.obolibrary.org/obo/GAZ_00239647"/>
        <obo:IAO_0000115>A suburb of Durban.</obo:IAO_0000115>
        <oboInOwl:hasOBONamespace>GAZ</oboInOwl:hasOBONamespace>
        <oboInOwl:id>GAZ:00239667</oboInOwl:id>
        <rdfs:label>Newlands</rdfs:label>
    </owl:NamedIndividual>
    


    <!-- http://purl.obolibrary.org/obo/GAZ_00239668 -->

    <owl:NamedIndividual rdf:about="http://purl.obolibrary.org/obo/GAZ_00239668">
        <obo:RO_0001025 rdf:resource="http://purl.obolibrary.org/obo/GAZ_00239647"/>
        <obo:IAO_0000115>A suburb of Durban.</obo:IAO_0000115>
        <oboInOwl:hasOBONamespace>GAZ</oboInOwl:hasOBONamespace>
        <oboInOwl:id>GAZ:00239668</oboInOwl:id>
        <rdfs:label>Overport</rdfs:label>
    </owl:NamedIndividual>
    


    <!-- http://purl.obolibrary.org/obo/GAZ_00239669 -->

    <owl:NamedIndividual rdf:about="http://purl.obolibrary.org/obo/GAZ_00239669">
        <obo:RO_0001025 rdf:resource="http://purl.obolibrary.org/obo/GAZ_00239647"/>
        <obo:IAO_0000115>A suburb of Durban.</obo:IAO_0000115>
        <oboInOwl:hasOBONamespace>GAZ</oboInOwl:hasOBONamespace>
        <oboInOwl:id>GAZ:00239669</oboInOwl:id>
        <rdfs:label>Phoenix</rdfs:label>
    </owl:NamedIndividual>
    


    <!-- http://purl.obolibrary.org/obo/GAZ_00239670 -->

    <owl:NamedIndividual rdf:about="http://purl.obolibrary.org/obo/GAZ_00239670">
        <obo:RO_0001025 rdf:resource="http://purl.obolibrary.org/obo/GAZ_00239647"/>
        <obo:IAO_0000115>A suburb of Durban.</obo:IAO_0000115>
        <oboInOwl:hasOBONamespace>GAZ</oboInOwl:hasOBONamespace>
        <oboInOwl:id>GAZ:00239670</oboInOwl:id>
        <rdfs:label>Puntans Hill</rdfs:label>
    </owl:NamedIndividual>
    


    <!-- http://purl.obolibrary.org/obo/GAZ_00239671 -->

    <owl:NamedIndividual rdf:about="http://purl.obolibrary.org/obo/GAZ_00239671">
        <obo:RO_0001025 rdf:resource="http://purl.obolibrary.org/obo/GAZ_00239647"/>
        <obo:IAO_0000115>A suburb of Durban.</obo:IAO_0000115>
        <oboInOwl:hasOBONamespace>GAZ</oboInOwl:hasOBONamespace>
        <oboInOwl:id>GAZ:00239671</oboInOwl:id>
        <rdfs:label>Springfield</rdfs:label>
    </owl:NamedIndividual>
    


    <!-- http://purl.obolibrary.org/obo/GAZ_00239672 -->

    <owl:NamedIndividual rdf:about="http://purl.obolibrary.org/obo/GAZ_00239672">
        <obo:RO_0001025 rdf:resource="http://purl.obolibrary.org/obo/GAZ_00239647"/>
        <obo:IAO_0000115>A suburb of Durban.</obo:IAO_0000115>
        <oboInOwl:hasOBONamespace>GAZ</oboInOwl:hasOBONamespace>
        <oboInOwl:id>GAZ:00239672</oboInOwl:id>
        <rdfs:label>Sydenham</rdfs:label>
    </owl:NamedIndividual>
    


    <!-- http://purl.obolibrary.org/obo/GAZ_00239673 -->

    <owl:NamedIndividual rdf:about="http://purl.obolibrary.org/obo/GAZ_00239673">
        <obo:RO_0001025 rdf:resource="http://purl.obolibrary.org/obo/GAZ_00239647"/>
        <obo:IAO_0000115>A suburb of Durban.</obo:IAO_0000115>
        <oboInOwl:hasOBONamespace>GAZ</oboInOwl:hasOBONamespace>
        <oboInOwl:id>GAZ:00239673</oboInOwl:id>
        <rdfs:label>Yellowwood Park</rdfs:label>
    </owl:NamedIndividual>
    


    <!-- http://purl.obolibrary.org/obo/GAZ_00239674 -->

    <owl:NamedIndividual rdf:about="http://purl.obolibrary.org/obo/GAZ_00239674">
        <obo:RO_0001025 rdf:resource="http://purl.obolibrary.org/obo/GAZ_00239648"/>
        <obo:IAO_0000115>A suburb of Durban.</obo:IAO_0000115>
        <oboInOwl:hasOBONamespace>GAZ</oboInOwl:hasOBONamespace>
        <oboInOwl:id>GAZ:00239674</oboInOwl:id>
        <rdfs:label>Bellair</rdfs:label>
    </owl:NamedIndividual>
    


    <!-- http://purl.obolibrary.org/obo/GAZ_00239675 -->

    <owl:NamedIndividual rdf:about="http://purl.obolibrary.org/obo/GAZ_00239675">
        <obo:RO_0001025 rdf:resource="http://purl.obolibrary.org/obo/GAZ_00239648"/>
        <obo:IAO_0000115>A suburb of Durban.</obo:IAO_0000115>
        <oboInOwl:hasOBONamespace>GAZ</oboInOwl:hasOBONamespace>
        <oboInOwl:id>GAZ:00239675</oboInOwl:id>
        <rdfs:label>Cato Manor</rdfs:label>
    </owl:NamedIndividual>
    


    <!-- http://purl.obolibrary.org/obo/GAZ_00239676 -->

    <owl:NamedIndividual rdf:about="http://purl.obolibrary.org/obo/GAZ_00239676">
        <obo:RO_0001025 rdf:resource="http://purl.obolibrary.org/obo/GAZ_00239648"/>
        <obo:IAO_0000115>A suburb of Durban.</obo:IAO_0000115>
        <oboInOwl:hasOBONamespace>GAZ</oboInOwl:hasOBONamespace>
        <oboInOwl:id>GAZ:00239676</oboInOwl:id>
        <rdfs:label>Chatsworth</rdfs:label>
    </owl:NamedIndividual>
    


    <!-- http://purl.obolibrary.org/obo/GAZ_00239677 -->

    <owl:NamedIndividual rdf:about="http://purl.obolibrary.org/obo/GAZ_00239677">
        <obo:RO_0001025 rdf:resource="http://purl.obolibrary.org/obo/GAZ_00239648"/>
        <obo:IAO_0000115>A suburb of Durban.</obo:IAO_0000115>
        <oboInOwl:hasOBONamespace>GAZ</oboInOwl:hasOBONamespace>
        <oboInOwl:id>GAZ:00239677</oboInOwl:id>
        <rdfs:label>Glen Park</rdfs:label>
    </owl:NamedIndividual>
    


    <!-- http://purl.obolibrary.org/obo/GAZ_00239678 -->

    <owl:NamedIndividual rdf:about="http://purl.obolibrary.org/obo/GAZ_00239678">
        <obo:RO_0001025 rdf:resource="http://purl.obolibrary.org/obo/GAZ_00239648"/>
        <obo:IAO_0000115>A suburb of Durban.</obo:IAO_0000115>
        <oboInOwl:hasOBONamespace>GAZ</oboInOwl:hasOBONamespace>
        <oboInOwl:id>GAZ:00239678</oboInOwl:id>
        <rdfs:label>Glenwood</rdfs:label>
    </owl:NamedIndividual>
    


    <!-- http://purl.obolibrary.org/obo/GAZ_00239679 -->

    <owl:NamedIndividual rdf:about="http://purl.obolibrary.org/obo/GAZ_00239679">
        <obo:RO_0001025 rdf:resource="http://purl.obolibrary.org/obo/GAZ_00239648"/>
        <obo:IAO_0000115>A suburb of Durban.</obo:IAO_0000115>
        <oboInOwl:hasOBONamespace>GAZ</oboInOwl:hasOBONamespace>
        <oboInOwl:id>GAZ:00239679</oboInOwl:id>
        <rdfs:label>Hillary</rdfs:label>
    </owl:NamedIndividual>
    


    <!-- http://purl.obolibrary.org/obo/GAZ_00239680 -->

    <owl:NamedIndividual rdf:about="http://purl.obolibrary.org/obo/GAZ_00239680">
        <obo:RO_0001025 rdf:resource="http://purl.obolibrary.org/obo/GAZ_00239648"/>
        <obo:IAO_0000115>A suburb of Durban.</obo:IAO_0000115>
        <oboInOwl:hasOBONamespace>GAZ</oboInOwl:hasOBONamespace>
        <oboInOwl:id>GAZ:00239680</oboInOwl:id>
        <rdfs:label>Jacobs Ladder</rdfs:label>
    </owl:NamedIndividual>
    


    <!-- http://purl.obolibrary.org/obo/GAZ_00239681 -->

    <owl:NamedIndividual rdf:about="http://purl.obolibrary.org/obo/GAZ_00239681">
        <obo:RO_0001025 rdf:resource="http://purl.obolibrary.org/obo/GAZ_00239648"/>
        <obo:IAO_0000115>A suburb of Durban.</obo:IAO_0000115>
        <oboInOwl:hasOBONamespace>GAZ</oboInOwl:hasOBONamespace>
        <oboInOwl:id>GAZ:00239681</oboInOwl:id>
        <rdfs:label>Memorial Park</rdfs:label>
    </owl:NamedIndividual>
    


    <!-- http://purl.obolibrary.org/obo/GAZ_00239682 -->

    <owl:NamedIndividual rdf:about="http://purl.obolibrary.org/obo/GAZ_00239682">
        <obo:RO_0001025 rdf:resource="http://purl.obolibrary.org/obo/GAZ_00239648"/>
        <obo:IAO_0000115>A suburb of Durban.</obo:IAO_0000115>
        <oboInOwl:hasOBONamespace>GAZ</oboInOwl:hasOBONamespace>
        <oboInOwl:id>GAZ:00239682</oboInOwl:id>
        <rdfs:label>Merebank</rdfs:label>
    </owl:NamedIndividual>
    


    <!-- http://purl.obolibrary.org/obo/GAZ_00239683 -->

    <owl:NamedIndividual rdf:about="http://purl.obolibrary.org/obo/GAZ_00239683">
        <obo:RO_0001025 rdf:resource="http://purl.obolibrary.org/obo/GAZ_00239648"/>
        <obo:IAO_0000115>A suburb of Durban.</obo:IAO_0000115>
        <oboInOwl:hasOBONamespace>GAZ</oboInOwl:hasOBONamespace>
        <oboInOwl:id>GAZ:00239683</oboInOwl:id>
        <rdfs:label>Merewent</rdfs:label>
    </owl:NamedIndividual>
    


    <!-- http://purl.obolibrary.org/obo/GAZ_00239684 -->

    <owl:NamedIndividual rdf:about="http://purl.obolibrary.org/obo/GAZ_00239684">
        <obo:RO_0001025 rdf:resource="http://purl.obolibrary.org/obo/GAZ_00239648"/>
        <obo:IAO_0000115>A suburb of Durban.</obo:IAO_0000115>
        <oboInOwl:hasOBONamespace>GAZ</oboInOwl:hasOBONamespace>
        <oboInOwl:id>GAZ:00239684</oboInOwl:id>
        <rdfs:label>Montclair</rdfs:label>
    </owl:NamedIndividual>
    


    <!-- http://purl.obolibrary.org/obo/GAZ_00239685 -->

    <owl:NamedIndividual rdf:about="http://purl.obolibrary.org/obo/GAZ_00239685">
        <obo:RO_0001025 rdf:resource="http://purl.obolibrary.org/obo/GAZ_00239648"/>
        <obo:IAO_0000115>A suburb of Durban.</obo:IAO_0000115>
        <oboInOwl:hasOBONamespace>GAZ</oboInOwl:hasOBONamespace>
        <oboInOwl:id>GAZ:00239685</oboInOwl:id>
        <rdfs:label>Mount Vernon</rdfs:label>
    </owl:NamedIndividual>
    


    <!-- http://purl.obolibrary.org/obo/GAZ_00239686 -->

    <owl:NamedIndividual rdf:about="http://purl.obolibrary.org/obo/GAZ_00239686">
        <obo:RO_0001025 rdf:resource="http://purl.obolibrary.org/obo/GAZ_00239648"/>
        <obo:IAO_0000115>A suburb of Durban.</obo:IAO_0000115>
        <oboInOwl:hasOBONamespace>GAZ</oboInOwl:hasOBONamespace>
        <oboInOwl:id>GAZ:00239686</oboInOwl:id>
        <rdfs:label>Northdene</rdfs:label>
    </owl:NamedIndividual>
    


    <!-- http://purl.obolibrary.org/obo/GAZ_00239687 -->

    <owl:NamedIndividual rdf:about="http://purl.obolibrary.org/obo/GAZ_00239687">
        <obo:RO_0001025 rdf:resource="http://purl.obolibrary.org/obo/GAZ_00239648"/>
        <obo:IAO_0000115>A suburb of Durban.</obo:IAO_0000115>
        <oboInOwl:hasOBONamespace>GAZ</oboInOwl:hasOBONamespace>
        <oboInOwl:id>GAZ:00239687</oboInOwl:id>
        <rdfs:label>North Park</rdfs:label>
    </owl:NamedIndividual>
    


    <!-- http://purl.obolibrary.org/obo/GAZ_00239688 -->

    <owl:NamedIndividual rdf:about="http://purl.obolibrary.org/obo/GAZ_00239688">
        <obo:RO_0001025 rdf:resource="http://purl.obolibrary.org/obo/GAZ_00239648"/>
        <obo:IAO_0000115>A suburb of Durban.</obo:IAO_0000115>
        <oboInOwl:hasOBONamespace>GAZ</oboInOwl:hasOBONamespace>
        <oboInOwl:id>GAZ:00239688</oboInOwl:id>
        <rdfs:label>Poets Corner</rdfs:label>
    </owl:NamedIndividual>
    


    <!-- http://purl.obolibrary.org/obo/GAZ_00239689 -->

    <owl:NamedIndividual rdf:about="http://purl.obolibrary.org/obo/GAZ_00239689">
        <obo:RO_0001025 rdf:resource="http://purl.obolibrary.org/obo/GAZ_00239648"/>
        <obo:IAO_0000115>A suburb of Durban.</obo:IAO_0000115>
        <oboInOwl:hasOBONamespace>GAZ</oboInOwl:hasOBONamespace>
        <oboInOwl:id>GAZ:00239689</oboInOwl:id>
        <rdfs:label>Prospecton</rdfs:label>
    </owl:NamedIndividual>
    


    <!-- http://purl.obolibrary.org/obo/GAZ_00239690 -->

    <owl:NamedIndividual rdf:about="http://purl.obolibrary.org/obo/GAZ_00239690">
        <obo:RO_0001025 rdf:resource="http://purl.obolibrary.org/obo/GAZ_00239648"/>
        <obo:IAO_0000115>A suburb of Durban.</obo:IAO_0000115>
        <oboInOwl:hasOBONamespace>GAZ</oboInOwl:hasOBONamespace>
        <oboInOwl:id>GAZ:00239690</oboInOwl:id>
        <rdfs:label>Rossburgh</rdfs:label>
    </owl:NamedIndividual>
    


    <!-- http://purl.obolibrary.org/obo/GAZ_00239691 -->

    <owl:NamedIndividual rdf:about="http://purl.obolibrary.org/obo/GAZ_00239691">
        <obo:RO_0001025 rdf:resource="http://purl.obolibrary.org/obo/GAZ_00239648"/>
        <obo:IAO_0000115>A suburb of Durban.</obo:IAO_0000115>
        <oboInOwl:hasOBONamespace>GAZ</oboInOwl:hasOBONamespace>
        <oboInOwl:id>GAZ:00239691</oboInOwl:id>
        <rdfs:label>Sarnia</rdfs:label>
    </owl:NamedIndividual>
    


    <!-- http://purl.obolibrary.org/obo/GAZ_00239692 -->

    <owl:NamedIndividual rdf:about="http://purl.obolibrary.org/obo/GAZ_00239692">
        <obo:RO_0001025 rdf:resource="http://purl.obolibrary.org/obo/GAZ_00239648"/>
        <obo:IAO_0000115>A suburb of Durban.</obo:IAO_0000115>
        <oboInOwl:hasOBONamespace>GAZ</oboInOwl:hasOBONamespace>
        <oboInOwl:id>GAZ:00239692</oboInOwl:id>
        <rdfs:label>Seaview</rdfs:label>
    </owl:NamedIndividual>
    


    <!-- http://purl.obolibrary.org/obo/GAZ_00239693 -->

    <owl:NamedIndividual rdf:about="http://purl.obolibrary.org/obo/GAZ_00239693">
        <obo:RO_0001025 rdf:resource="http://purl.obolibrary.org/obo/GAZ_00239648"/>
        <obo:IAO_0000115>A suburb of Durban.</obo:IAO_0000115>
        <oboInOwl:hasOBONamespace>GAZ</oboInOwl:hasOBONamespace>
        <oboInOwl:id>GAZ:00239693</oboInOwl:id>
        <rdfs:label>Shallcross</rdfs:label>
    </owl:NamedIndividual>
    


    <!-- http://purl.obolibrary.org/obo/GAZ_00239694 -->

    <owl:NamedIndividual rdf:about="http://purl.obolibrary.org/obo/GAZ_00239694">
        <obo:RO_0001025 rdf:resource="http://purl.obolibrary.org/obo/GAZ_00239648"/>
        <obo:IAO_0000115>A suburb of Durban.</obo:IAO_0000115>
        <oboInOwl:hasOBONamespace>GAZ</oboInOwl:hasOBONamespace>
        <oboInOwl:id>GAZ:00239694</oboInOwl:id>
        <rdfs:label>Treasure Beach</rdfs:label>
    </owl:NamedIndividual>
    


    <!-- http://purl.obolibrary.org/obo/GAZ_00239695 -->

    <owl:NamedIndividual rdf:about="http://purl.obolibrary.org/obo/GAZ_00239695">
        <obo:RO_0001025 rdf:resource="http://purl.obolibrary.org/obo/GAZ_00239648"/>
        <obo:IAO_0000115>A suburb of Durban.</obo:IAO_0000115>
        <oboInOwl:hasOBONamespace>GAZ</oboInOwl:hasOBONamespace>
        <oboInOwl:id>GAZ:00239695</oboInOwl:id>
        <rdfs:label>Wentworth</rdfs:label>
    </owl:NamedIndividual>
    


    <!-- http://purl.obolibrary.org/obo/GAZ_00239696 -->

    <owl:NamedIndividual rdf:about="http://purl.obolibrary.org/obo/GAZ_00239696">
        <obo:RO_0001025 rdf:resource="http://purl.obolibrary.org/obo/GAZ_00239648"/>
        <obo:IAO_0000115>A suburb of Durban.</obo:IAO_0000115>
        <oboInOwl:hasOBONamespace>GAZ</oboInOwl:hasOBONamespace>
        <oboInOwl:id>GAZ:00239696</oboInOwl:id>
        <rdfs:label>Umhlatuzana</rdfs:label>
    </owl:NamedIndividual>
    


    <!-- http://purl.obolibrary.org/obo/GAZ_00239697 -->

    <owl:NamedIndividual rdf:about="http://purl.obolibrary.org/obo/GAZ_00239697">
        <obo:RO_0001025 rdf:resource="http://purl.obolibrary.org/obo/GAZ_00239648"/>
        <obo:IAO_0000115>A suburb of Durban.</obo:IAO_0000115>
        <oboInOwl:hasOBONamespace>GAZ</oboInOwl:hasOBONamespace>
        <oboInOwl:id>GAZ:00239697</oboInOwl:id>
        <rdfs:label>Umlazi</rdfs:label>
    </owl:NamedIndividual>
    


    <!-- http://purl.obolibrary.org/obo/GAZ_00239698 -->

    <owl:NamedIndividual rdf:about="http://purl.obolibrary.org/obo/GAZ_00239698">
        <obo:RO_0001025 rdf:resource="http://purl.obolibrary.org/obo/GAZ_00239648"/>
        <obo:IAO_0000115>A suburb of Durban.</obo:IAO_0000115>
        <oboInOwl:hasOBONamespace>GAZ</oboInOwl:hasOBONamespace>
        <oboInOwl:id>GAZ:00239698</oboInOwl:id>
        <rdfs:label>Umbilo</rdfs:label>
    </owl:NamedIndividual>
    


    <!-- http://purl.obolibrary.org/obo/GAZ_00239699 -->

    <owl:NamedIndividual rdf:about="http://purl.obolibrary.org/obo/GAZ_00239699">
        <obo:RO_0001025 rdf:resource="http://purl.obolibrary.org/obo/GAZ_00239648"/>
        <obo:IAO_0000115>A suburb of Durban.</obo:IAO_0000115>
        <oboInOwl:hasOBONamespace>GAZ</oboInOwl:hasOBONamespace>
        <oboInOwl:id>GAZ:00239699</oboInOwl:id>
        <rdfs:label>Woodhaven</rdfs:label>
    </owl:NamedIndividual>
    


    <!-- http://purl.obolibrary.org/obo/GAZ_00239700 -->

    <owl:NamedIndividual rdf:about="http://purl.obolibrary.org/obo/GAZ_00239700">
        <obo:RO_0001025 rdf:resource="http://purl.obolibrary.org/obo/GAZ_00239648"/>
        <obo:IAO_0000115>A suburb of Durban.</obo:IAO_0000115>
        <oboInOwl:hasOBONamespace>GAZ</oboInOwl:hasOBONamespace>
        <oboInOwl:id>GAZ:00239700</oboInOwl:id>
        <rdfs:label>Woodlands</rdfs:label>
    </owl:NamedIndividual>
    


    <!-- http://purl.obolibrary.org/obo/GAZ_00239701 -->

    <owl:NamedIndividual rdf:about="http://purl.obolibrary.org/obo/GAZ_00239701">
        <obo:RO_0001025 rdf:resource="http://purl.obolibrary.org/obo/GAZ_00239648"/>
        <obo:IAO_0000115>A suburb of Durban.</obo:IAO_0000115>
        <oboInOwl:hasOBONamespace>GAZ</oboInOwl:hasOBONamespace>
        <oboInOwl:id>GAZ:00239701</oboInOwl:id>
        <rdfs:label>Yellowood Park</rdfs:label>
    </owl:NamedIndividual>
    


    <!-- http://purl.obolibrary.org/obo/GAZ_00239702 -->

    <owl:NamedIndividual rdf:about="http://purl.obolibrary.org/obo/GAZ_00239702">
        <obo:RO_0001025 rdf:resource="http://purl.obolibrary.org/obo/GAZ_00239650"/>
        <obo:IAO_0000115>A suburb of Durban.</obo:IAO_0000115>
        <oboInOwl:hasOBONamespace>GAZ</oboInOwl:hasOBONamespace>
        <oboInOwl:id>GAZ:00239702</oboInOwl:id>
        <rdfs:label>Alverstone</rdfs:label>
    </owl:NamedIndividual>
    


    <!-- http://purl.obolibrary.org/obo/GAZ_00239703 -->

    <owl:NamedIndividual rdf:about="http://purl.obolibrary.org/obo/GAZ_00239703">
        <obo:RO_0001025 rdf:resource="http://purl.obolibrary.org/obo/GAZ_00239650"/>
        <obo:IAO_0000115>A suburb of Durban.</obo:IAO_0000115>
        <oboInOwl:hasOBONamespace>GAZ</oboInOwl:hasOBONamespace>
        <oboInOwl:id>GAZ:00239703</oboInOwl:id>
        <rdfs:label>Assagay</rdfs:label>
    </owl:NamedIndividual>
    


    <!-- http://purl.obolibrary.org/obo/GAZ_00239704 -->

    <owl:NamedIndividual rdf:about="http://purl.obolibrary.org/obo/GAZ_00239704">
        <obo:RO_0001025 rdf:resource="http://purl.obolibrary.org/obo/GAZ_00239650"/>
        <obo:IAO_0000115>A suburb of Durban.</obo:IAO_0000115>
        <oboInOwl:hasOBONamespace>GAZ</oboInOwl:hasOBONamespace>
        <oboInOwl:id>GAZ:00239704</oboInOwl:id>
        <rdfs:label>Botha&apos;s Hill</rdfs:label>
    </owl:NamedIndividual>
    


    <!-- http://purl.obolibrary.org/obo/GAZ_00239705 -->

    <owl:NamedIndividual rdf:about="http://purl.obolibrary.org/obo/GAZ_00239705">
        <obo:RO_0001025 rdf:resource="http://purl.obolibrary.org/obo/GAZ_00239650"/>
        <obo:IAO_0000115>A suburb of Durban.</obo:IAO_0000115>
        <oboInOwl:hasOBONamespace>GAZ</oboInOwl:hasOBONamespace>
        <oboInOwl:id>GAZ:00239705</oboInOwl:id>
        <rdfs:label>Cato Ridge</rdfs:label>
    </owl:NamedIndividual>
    


    <!-- http://purl.obolibrary.org/obo/GAZ_00239706 -->

    <owl:NamedIndividual rdf:about="http://purl.obolibrary.org/obo/GAZ_00239706">
        <obo:RO_0001025 rdf:resource="http://purl.obolibrary.org/obo/GAZ_00239650"/>
        <obo:IAO_0000115>A suburb of Durban.</obo:IAO_0000115>
        <oboInOwl:hasOBONamespace>GAZ</oboInOwl:hasOBONamespace>
        <oboInOwl:id>GAZ:00239706</oboInOwl:id>
        <rdfs:label>Crestholm</rdfs:label>
    </owl:NamedIndividual>
    


    <!-- http://purl.obolibrary.org/obo/GAZ_00239707 -->

    <owl:NamedIndividual rdf:about="http://purl.obolibrary.org/obo/GAZ_00239707">
        <obo:RO_0001025 rdf:resource="http://purl.obolibrary.org/obo/GAZ_00239650"/>
        <obo:IAO_0000115>A suburb of Durban.</obo:IAO_0000115>
        <oboInOwl:hasOBONamespace>GAZ</oboInOwl:hasOBONamespace>
        <oboInOwl:id>GAZ:00239707</oboInOwl:id>
        <rdfs:label>Cliffdale</rdfs:label>
    </owl:NamedIndividual>
    


    <!-- http://purl.obolibrary.org/obo/GAZ_00239708 -->

    <owl:NamedIndividual rdf:about="http://purl.obolibrary.org/obo/GAZ_00239708">
        <obo:RO_0001025 rdf:resource="http://purl.obolibrary.org/obo/GAZ_00239650"/>
        <obo:IAO_0000115>A suburb of Durban.</obo:IAO_0000115>
        <oboInOwl:hasOBONamespace>GAZ</oboInOwl:hasOBONamespace>
        <oboInOwl:id>GAZ:00239708</oboInOwl:id>
        <rdfs:label>Clifton Canyon</rdfs:label>
    </owl:NamedIndividual>
    


    <!-- http://purl.obolibrary.org/obo/GAZ_00239709 -->

    <owl:NamedIndividual rdf:about="http://purl.obolibrary.org/obo/GAZ_00239709">
        <obo:RO_0001025 rdf:resource="http://purl.obolibrary.org/obo/GAZ_00239650"/>
        <obo:IAO_0000115>A suburb of Durban.</obo:IAO_0000115>
        <oboInOwl:hasOBONamespace>GAZ</oboInOwl:hasOBONamespace>
        <oboInOwl:id>GAZ:00239709</oboInOwl:id>
        <rdfs:label>Drummond</rdfs:label>
    </owl:NamedIndividual>
    


    <!-- http://purl.obolibrary.org/obo/GAZ_00239710 -->

    <owl:NamedIndividual rdf:about="http://purl.obolibrary.org/obo/GAZ_00239710">
        <obo:RO_0001025 rdf:resource="http://purl.obolibrary.org/obo/GAZ_00239650"/>
        <obo:IAO_0000115>A suburb of Durban.</obo:IAO_0000115>
        <oboInOwl:hasOBONamespace>GAZ</oboInOwl:hasOBONamespace>
        <oboInOwl:id>GAZ:00239710</oboInOwl:id>
        <rdfs:label>Everton</rdfs:label>
    </owl:NamedIndividual>
    


    <!-- http://purl.obolibrary.org/obo/GAZ_00239711 -->

    <owl:NamedIndividual rdf:about="http://purl.obolibrary.org/obo/GAZ_00239711">
        <obo:RO_0001025 rdf:resource="http://purl.obolibrary.org/obo/GAZ_00239650"/>
        <obo:IAO_0000115>A suburb of Durban.</obo:IAO_0000115>
        <oboInOwl:hasOBONamespace>GAZ</oboInOwl:hasOBONamespace>
        <oboInOwl:id>GAZ:00239711</oboInOwl:id>
        <rdfs:label>Emberton</rdfs:label>
    </owl:NamedIndividual>
    


    <!-- http://purl.obolibrary.org/obo/GAZ_00239712 -->

    <owl:NamedIndividual rdf:about="http://purl.obolibrary.org/obo/GAZ_00239712">
        <obo:RO_0001025 rdf:resource="http://purl.obolibrary.org/obo/GAZ_00239650"/>
        <obo:IAO_0000115>A suburb of Durban.</obo:IAO_0000115>
        <oboInOwl:hasOBONamespace>GAZ</oboInOwl:hasOBONamespace>
        <oboInOwl:id>GAZ:00239712</oboInOwl:id>
        <rdfs:label>Forest Hills</rdfs:label>
    </owl:NamedIndividual>
    


    <!-- http://purl.obolibrary.org/obo/GAZ_00239713 -->

    <owl:NamedIndividual rdf:about="http://purl.obolibrary.org/obo/GAZ_00239713">
        <obo:RO_0001025 rdf:resource="http://purl.obolibrary.org/obo/GAZ_00239650"/>
        <obo:IAO_0000115>A suburb of Durban.</obo:IAO_0000115>
        <oboInOwl:hasOBONamespace>GAZ</oboInOwl:hasOBONamespace>
        <oboInOwl:id>GAZ:00239713</oboInOwl:id>
        <rdfs:label>Fredville</rdfs:label>
    </owl:NamedIndividual>
    


    <!-- http://purl.obolibrary.org/obo/GAZ_00239714 -->

    <owl:NamedIndividual rdf:about="http://purl.obolibrary.org/obo/GAZ_00239714">
        <obo:RO_0001025 rdf:resource="http://purl.obolibrary.org/obo/GAZ_00239650"/>
        <obo:IAO_0000115>A suburb of Durban.</obo:IAO_0000115>
        <oboInOwl:hasOBONamespace>GAZ</oboInOwl:hasOBONamespace>
        <oboInOwl:id>GAZ:00239714</oboInOwl:id>
        <rdfs:label>Gillitts</rdfs:label>
    </owl:NamedIndividual>
    


    <!-- http://purl.obolibrary.org/obo/GAZ_00239715 -->

    <owl:NamedIndividual rdf:about="http://purl.obolibrary.org/obo/GAZ_00239715">
        <obo:RO_0001025 rdf:resource="http://purl.obolibrary.org/obo/GAZ_00239650"/>
        <obo:IAO_0000115>A suburb of Durban.</obo:IAO_0000115>
        <oboInOwl:hasOBONamespace>GAZ</oboInOwl:hasOBONamespace>
        <oboInOwl:id>GAZ:00239715</oboInOwl:id>
        <rdfs:label>Hammarsdale</rdfs:label>
    </owl:NamedIndividual>
    


    <!-- http://purl.obolibrary.org/obo/GAZ_00239716 -->

    <owl:NamedIndividual rdf:about="http://purl.obolibrary.org/obo/GAZ_00239716">
        <obo:RO_0001025 rdf:resource="http://purl.obolibrary.org/obo/GAZ_00239650"/>
        <obo:IAO_0000115>A suburb of Durban.</obo:IAO_0000115>
        <oboInOwl:hasOBONamespace>GAZ</oboInOwl:hasOBONamespace>
        <oboInOwl:id>GAZ:00239716</oboInOwl:id>
        <rdfs:label>Harrison</rdfs:label>
    </owl:NamedIndividual>
    


    <!-- http://purl.obolibrary.org/obo/GAZ_00239717 -->

    <owl:NamedIndividual rdf:about="http://purl.obolibrary.org/obo/GAZ_00239717">
        <obo:RO_0001025 rdf:resource="http://purl.obolibrary.org/obo/GAZ_00239650"/>
        <obo:IAO_0000115>A suburb of Durban.</obo:IAO_0000115>
        <oboInOwl:hasOBONamespace>GAZ</oboInOwl:hasOBONamespace>
        <oboInOwl:id>GAZ:00239717</oboInOwl:id>
        <rdfs:label>Hillcrest</rdfs:label>
    </owl:NamedIndividual>
    


    <!-- http://purl.obolibrary.org/obo/GAZ_00239718 -->

    <owl:NamedIndividual rdf:about="http://purl.obolibrary.org/obo/GAZ_00239718">
        <obo:RO_0001025 rdf:resource="http://purl.obolibrary.org/obo/GAZ_00239650"/>
        <obo:IAO_0000115>A suburb of Durban.</obo:IAO_0000115>
        <oboInOwl:hasOBONamespace>GAZ</oboInOwl:hasOBONamespace>
        <oboInOwl:id>GAZ:00239718</oboInOwl:id>
        <rdfs:label>Inchanga</rdfs:label>
    </owl:NamedIndividual>
    


    <!-- http://purl.obolibrary.org/obo/GAZ_00239719 -->

    <owl:NamedIndividual rdf:about="http://purl.obolibrary.org/obo/GAZ_00239719">
        <obo:RO_0001025 rdf:resource="http://purl.obolibrary.org/obo/GAZ_00239650"/>
        <obo:IAO_0000115>A suburb of Durban.</obo:IAO_0000115>
        <oboInOwl:hasOBONamespace>GAZ</oboInOwl:hasOBONamespace>
        <oboInOwl:id>GAZ:00239719</oboInOwl:id>
        <rdfs:label>Kloof</rdfs:label>
    </owl:NamedIndividual>
    


    <!-- http://purl.obolibrary.org/obo/GAZ_00239720 -->

    <owl:NamedIndividual rdf:about="http://purl.obolibrary.org/obo/GAZ_00239720">
        <obo:RO_0001025 rdf:resource="http://purl.obolibrary.org/obo/GAZ_00239650"/>
        <obo:IAO_0000115>A suburb of Durban.</obo:IAO_0000115>
        <oboInOwl:hasOBONamespace>GAZ</oboInOwl:hasOBONamespace>
        <oboInOwl:id>GAZ:00239720</oboInOwl:id>
        <rdfs:label>KwaXimba</rdfs:label>
    </owl:NamedIndividual>
    


    <!-- http://purl.obolibrary.org/obo/GAZ_00239721 -->

    <owl:NamedIndividual rdf:about="http://purl.obolibrary.org/obo/GAZ_00239721">
        <obo:RO_0001025 rdf:resource="http://purl.obolibrary.org/obo/GAZ_00239650"/>
        <obo:IAO_0000115>A suburb of Durban.</obo:IAO_0000115>
        <oboInOwl:hasOBONamespace>GAZ</oboInOwl:hasOBONamespace>
        <oboInOwl:id>GAZ:00239721</oboInOwl:id>
        <rdfs:label>Molweni</rdfs:label>
    </owl:NamedIndividual>
    


    <!-- http://purl.obolibrary.org/obo/GAZ_00239722 -->

    <owl:NamedIndividual rdf:about="http://purl.obolibrary.org/obo/GAZ_00239722">
        <obo:RO_0001025 rdf:resource="http://purl.obolibrary.org/obo/GAZ_00239650"/>
        <obo:IAO_0000115>A suburb of Durban.</obo:IAO_0000115>
        <oboInOwl:hasOBONamespace>GAZ</oboInOwl:hasOBONamespace>
        <oboInOwl:id>GAZ:00239722</oboInOwl:id>
        <rdfs:label>Monteseel</rdfs:label>
    </owl:NamedIndividual>
    


    <!-- http://purl.obolibrary.org/obo/GAZ_00239723 -->

    <owl:NamedIndividual rdf:about="http://purl.obolibrary.org/obo/GAZ_00239723">
        <obo:RO_0001025 rdf:resource="http://purl.obolibrary.org/obo/GAZ_00239650"/>
        <obo:IAO_0000115>A suburb of Durban.</obo:IAO_0000115>
        <oboInOwl:hasOBONamespace>GAZ</oboInOwl:hasOBONamespace>
        <oboInOwl:id>GAZ:00239723</oboInOwl:id>
        <rdfs:label>Mpumalanga</rdfs:label>
    </owl:NamedIndividual>
    


    <!-- http://purl.obolibrary.org/obo/GAZ_00239724 -->

    <owl:NamedIndividual rdf:about="http://purl.obolibrary.org/obo/GAZ_00239724">
        <obo:RO_0001025 rdf:resource="http://purl.obolibrary.org/obo/GAZ_00239650"/>
        <obo:IAO_0000115>A suburb of Durban.</obo:IAO_0000115>
        <oboInOwl:hasOBONamespace>GAZ</oboInOwl:hasOBONamespace>
        <oboInOwl:id>GAZ:00239724</oboInOwl:id>
        <rdfs:label>Peacevale</rdfs:label>
    </owl:NamedIndividual>
    


    <!-- http://purl.obolibrary.org/obo/GAZ_00239725 -->

    <owl:NamedIndividual rdf:about="http://purl.obolibrary.org/obo/GAZ_00239725">
        <obo:RO_0001025 rdf:resource="http://purl.obolibrary.org/obo/GAZ_00239650"/>
        <obo:IAO_0000115>A suburb of Durban.</obo:IAO_0000115>
        <oboInOwl:hasOBONamespace>GAZ</oboInOwl:hasOBONamespace>
        <oboInOwl:id>GAZ:00239725</oboInOwl:id>
        <rdfs:label>Shongweni</rdfs:label>
    </owl:NamedIndividual>
    


    <!-- http://purl.obolibrary.org/obo/GAZ_00239726 -->

    <owl:NamedIndividual rdf:about="http://purl.obolibrary.org/obo/GAZ_00239726">
        <obo:RO_0001025 rdf:resource="http://purl.obolibrary.org/obo/GAZ_00239650"/>
        <obo:IAO_0000115>A suburb of Durban.</obo:IAO_0000115>
        <oboInOwl:hasOBONamespace>GAZ</oboInOwl:hasOBONamespace>
        <oboInOwl:id>GAZ:00239726</oboInOwl:id>
        <rdfs:label>Summerveld</rdfs:label>
    </owl:NamedIndividual>
    


    <!-- http://purl.obolibrary.org/obo/GAZ_00239727 -->

    <owl:NamedIndividual rdf:about="http://purl.obolibrary.org/obo/GAZ_00239727">
        <obo:RO_0001025 rdf:resource="http://purl.obolibrary.org/obo/GAZ_00239650"/>
        <obo:IAO_0000115>A suburb of Durban.</obo:IAO_0000115>
        <oboInOwl:hasOBONamespace>GAZ</oboInOwl:hasOBONamespace>
        <oboInOwl:id>GAZ:00239727</oboInOwl:id>
        <rdfs:label>Waterfall</rdfs:label>
    </owl:NamedIndividual>
    


    <!-- http://purl.obolibrary.org/obo/GAZ_00239728 -->

    <owl:NamedIndividual rdf:about="http://purl.obolibrary.org/obo/GAZ_00239728">
        <obo:RO_0001025 rdf:resource="http://purl.obolibrary.org/obo/GAZ_00239650"/>
        <obo:IAO_0000115>A suburb of Durban.</obo:IAO_0000115>
        <oboInOwl:hasOBONamespace>GAZ</oboInOwl:hasOBONamespace>
        <oboInOwl:id>GAZ:00239728</oboInOwl:id>
        <rdfs:label>Winston Park</rdfs:label>
    </owl:NamedIndividual>
    


    <!-- http://purl.obolibrary.org/obo/GAZ_00239729 -->

    <owl:NamedIndividual rdf:about="http://purl.obolibrary.org/obo/GAZ_00239729">
        <obo:RO_0001025 rdf:resource="http://purl.obolibrary.org/obo/GAZ_00239650"/>
        <obo:IAO_0000115>A suburb of Durban.</obo:IAO_0000115>
        <oboInOwl:hasOBONamespace>GAZ</oboInOwl:hasOBONamespace>
        <oboInOwl:id>GAZ:00239729</oboInOwl:id>
        <rdfs:label>Wyebank</rdfs:label>
    </owl:NamedIndividual>
    


    <!-- http://purl.obolibrary.org/obo/GAZ_00239730 -->

    <owl:NamedIndividual rdf:about="http://purl.obolibrary.org/obo/GAZ_00239730">
        <obo:RO_0001025 rdf:resource="http://purl.obolibrary.org/obo/GAZ_00239649"/>
        <obo:IAO_0000115>A suburb of Durban.</obo:IAO_0000115>
        <oboInOwl:hasOBONamespace>GAZ</oboInOwl:hasOBONamespace>
        <oboInOwl:id>GAZ:00239730</oboInOwl:id>
        <rdfs:label>Canelands</rdfs:label>
    </owl:NamedIndividual>
    


    <!-- http://purl.obolibrary.org/obo/GAZ_00239731 -->

    <owl:NamedIndividual rdf:about="http://purl.obolibrary.org/obo/GAZ_00239731">
        <obo:RO_0001025 rdf:resource="http://purl.obolibrary.org/obo/GAZ_00239649"/>
        <obo:IAO_0000115>A suburb of Durban.</obo:IAO_0000115>
        <oboInOwl:hasOBONamespace>GAZ</oboInOwl:hasOBONamespace>
        <oboInOwl:id>GAZ:00239731</oboInOwl:id>
        <rdfs:label>Glen Anil</rdfs:label>
    </owl:NamedIndividual>
    


    <!-- http://purl.obolibrary.org/obo/GAZ_00239732 -->

    <owl:NamedIndividual rdf:about="http://purl.obolibrary.org/obo/GAZ_00239732">
        <obo:RO_0001025 rdf:resource="http://purl.obolibrary.org/obo/GAZ_00239649"/>
        <obo:IAO_0000115>A suburb of Durban.</obo:IAO_0000115>
        <oboInOwl:hasOBONamespace>GAZ</oboInOwl:hasOBONamespace>
        <oboInOwl:id>GAZ:00239732</oboInOwl:id>
        <rdfs:label>Hambanati</rdfs:label>
    </owl:NamedIndividual>
    


    <!-- http://purl.obolibrary.org/obo/GAZ_00239733 -->

    <owl:NamedIndividual rdf:about="http://purl.obolibrary.org/obo/GAZ_00239733">
        <obo:RO_0001025 rdf:resource="http://purl.obolibrary.org/obo/GAZ_00239649"/>
        <obo:IAO_0000115>A suburb of Durban.</obo:IAO_0000115>
        <oboInOwl:hasOBONamespace>GAZ</oboInOwl:hasOBONamespace>
        <oboInOwl:id>GAZ:00239733</oboInOwl:id>
        <rdfs:label>La Lucia</rdfs:label>
    </owl:NamedIndividual>
    


    <!-- http://purl.obolibrary.org/obo/GAZ_00239734 -->

    <owl:NamedIndividual rdf:about="http://purl.obolibrary.org/obo/GAZ_00239734">
        <obo:RO_0001025 rdf:resource="http://purl.obolibrary.org/obo/GAZ_00239649"/>
        <obo:IAO_0000115>A suburb of Durban.</obo:IAO_0000115>
        <oboInOwl:hasOBONamespace>GAZ</oboInOwl:hasOBONamespace>
        <oboInOwl:id>GAZ:00239734</oboInOwl:id>
        <rdfs:label>Mount Edgecombe</rdfs:label>
    </owl:NamedIndividual>
    


    <!-- http://purl.obolibrary.org/obo/GAZ_00239735 -->

    <owl:NamedIndividual rdf:about="http://purl.obolibrary.org/obo/GAZ_00239735">
        <obo:RO_0001025 rdf:resource="http://purl.obolibrary.org/obo/GAZ_00239649"/>
        <obo:IAO_0000115>A suburb of Durban.</obo:IAO_0000115>
        <oboInOwl:hasOBONamespace>GAZ</oboInOwl:hasOBONamespace>
        <oboInOwl:id>GAZ:00239735</oboInOwl:id>
        <rdfs:label>Verulam</rdfs:label>
    </owl:NamedIndividual>
    


    <!-- http://purl.obolibrary.org/obo/GAZ_00239736 -->

    <owl:NamedIndividual rdf:about="http://purl.obolibrary.org/obo/GAZ_00239736">
        <obo:RO_0001025 rdf:resource="http://purl.obolibrary.org/obo/GAZ_00239649"/>
        <obo:IAO_0000115>A suburb of Durban.</obo:IAO_0000115>
        <oboInOwl:hasOBONamespace>GAZ</oboInOwl:hasOBONamespace>
        <oboInOwl:id>GAZ:00239736</oboInOwl:id>
        <rdfs:label>Redcliffe</rdfs:label>
    </owl:NamedIndividual>
    


    <!-- http://purl.obolibrary.org/obo/GAZ_00239737 -->

    <owl:NamedIndividual rdf:about="http://purl.obolibrary.org/obo/GAZ_00239737">
        <obo:RO_0001025 rdf:resource="http://purl.obolibrary.org/obo/GAZ_00239649"/>
        <obo:IAO_0000115>A suburb of Durban.</obo:IAO_0000115>
        <oboInOwl:hasOBONamespace>GAZ</oboInOwl:hasOBONamespace>
        <oboInOwl:id>GAZ:00239737</oboInOwl:id>
        <rdfs:label>Tongaat</rdfs:label>
    </owl:NamedIndividual>
    


    <!-- http://purl.obolibrary.org/obo/GAZ_00239738 -->

    <owl:NamedIndividual rdf:about="http://purl.obolibrary.org/obo/GAZ_00239738">
        <obo:RO_0001025 rdf:resource="http://purl.obolibrary.org/obo/GAZ_00239649"/>
        <obo:IAO_0000115>A suburb of Durban.</obo:IAO_0000115>
        <oboInOwl:hasOBONamespace>GAZ</oboInOwl:hasOBONamespace>
        <oboInOwl:id>GAZ:00239738</oboInOwl:id>
        <rdfs:label>Umdloti</rdfs:label>
    </owl:NamedIndividual>
    


    <!-- http://purl.obolibrary.org/obo/GAZ_00239739 -->

    <owl:NamedIndividual rdf:about="http://purl.obolibrary.org/obo/GAZ_00239739">
        <obo:RO_0001025 rdf:resource="http://purl.obolibrary.org/obo/GAZ_00239649"/>
        <obo:IAO_0000115>A residential, commercial and resort town north of Durban on the coast of KwaZulu-Natal, South Africa.</obo:IAO_0000115>
        <oboInOwl:hasOBONamespace>GAZ</oboInOwl:hasOBONamespace>
        <oboInOwl:id>GAZ:00239739</oboInOwl:id>
        <rdfs:label>Umhlanga</rdfs:label>
    </owl:NamedIndividual>
    


    <!-- http://purl.obolibrary.org/obo/GAZ_00239741 -->

    <owl:NamedIndividual rdf:about="http://purl.obolibrary.org/obo/GAZ_00239741">
        <obo:RO_0001025 rdf:resource="http://purl.obolibrary.org/obo/GAZ_00239651"/>
        <obo:IAO_0000115>A suburb of Durban.</obo:IAO_0000115>
        <oboInOwl:hasOBONamespace>GAZ</oboInOwl:hasOBONamespace>
        <oboInOwl:id>GAZ:00239741</oboInOwl:id>
        <rdfs:label>Berea West</rdfs:label>
    </owl:NamedIndividual>
    


    <!-- http://purl.obolibrary.org/obo/GAZ_00239742 -->

    <owl:NamedIndividual rdf:about="http://purl.obolibrary.org/obo/GAZ_00239742">
        <obo:RO_0001025 rdf:resource="http://purl.obolibrary.org/obo/GAZ_00239651"/>
        <obo:IAO_0000115>A suburb of Durban.</obo:IAO_0000115>
        <oboInOwl:hasOBONamespace>GAZ</oboInOwl:hasOBONamespace>
        <oboInOwl:id>GAZ:00239742</oboInOwl:id>
        <rdfs:label>Chiltern Hills</rdfs:label>
    </owl:NamedIndividual>
    


    <!-- http://purl.obolibrary.org/obo/GAZ_00239743 -->

    <owl:NamedIndividual rdf:about="http://purl.obolibrary.org/obo/GAZ_00239743">
        <obo:RO_0001025 rdf:resource="http://purl.obolibrary.org/obo/GAZ_00239651"/>
        <obo:IAO_0000115>A suburb of Durban.</obo:IAO_0000115>
        <oboInOwl:hasOBONamespace>GAZ</oboInOwl:hasOBONamespace>
        <oboInOwl:id>GAZ:00239743</oboInOwl:id>
        <rdfs:label>Clermont</rdfs:label>
    </owl:NamedIndividual>
    


    <!-- http://purl.obolibrary.org/obo/GAZ_00239744 -->

    <owl:NamedIndividual rdf:about="http://purl.obolibrary.org/obo/GAZ_00239744">
        <obo:RO_0001025 rdf:resource="http://purl.obolibrary.org/obo/GAZ_00239651"/>
        <obo:IAO_0000115>A suburb of Durban.</obo:IAO_0000115>
        <oboInOwl:hasOBONamespace>GAZ</oboInOwl:hasOBONamespace>
        <oboInOwl:id>GAZ:00239744</oboInOwl:id>
        <rdfs:label>Cowies Hill</rdfs:label>
    </owl:NamedIndividual>
    


    <!-- http://purl.obolibrary.org/obo/GAZ_00239745 -->

    <owl:NamedIndividual rdf:about="http://purl.obolibrary.org/obo/GAZ_00239745">
        <obo:RO_0001025 rdf:resource="http://purl.obolibrary.org/obo/GAZ_00239651"/>
        <obo:IAO_0000115>A suburb of Durban.</obo:IAO_0000115>
        <oboInOwl:hasOBONamespace>GAZ</oboInOwl:hasOBONamespace>
        <oboInOwl:id>GAZ:00239745</oboInOwl:id>
        <rdfs:label>Dassenhoek</rdfs:label>
    </owl:NamedIndividual>
    


    <!-- http://purl.obolibrary.org/obo/GAZ_00239746 -->

    <owl:NamedIndividual rdf:about="http://purl.obolibrary.org/obo/GAZ_00239746">
        <obo:RO_0001025 rdf:resource="http://purl.obolibrary.org/obo/GAZ_00239651"/>
        <obo:IAO_0000115>A suburb of Durban.</obo:IAO_0000115>
        <oboInOwl:hasOBONamespace>GAZ</oboInOwl:hasOBONamespace>
        <oboInOwl:id>GAZ:00239746</oboInOwl:id>
        <rdfs:label>Klaarwater</rdfs:label>
    </owl:NamedIndividual>
    


    <!-- http://purl.obolibrary.org/obo/GAZ_00239747 -->

    <owl:NamedIndividual rdf:about="http://purl.obolibrary.org/obo/GAZ_00239747">
        <obo:RO_0001025 rdf:resource="http://purl.obolibrary.org/obo/GAZ_00239651"/>
        <obo:IAO_0000115>A suburb of Durban.</obo:IAO_0000115>
        <oboInOwl:hasOBONamespace>GAZ</oboInOwl:hasOBONamespace>
        <oboInOwl:id>GAZ:00239747</oboInOwl:id>
        <rdfs:label>KwaDabeka</rdfs:label>
    </owl:NamedIndividual>
    


    <!-- http://purl.obolibrary.org/obo/GAZ_00239748 -->

    <owl:NamedIndividual rdf:about="http://purl.obolibrary.org/obo/GAZ_00239748">
        <obo:RO_0001025 rdf:resource="http://purl.obolibrary.org/obo/GAZ_00239651"/>
        <obo:IAO_0000115>A suburb of Durban.</obo:IAO_0000115>
        <oboInOwl:hasOBONamespace>GAZ</oboInOwl:hasOBONamespace>
        <oboInOwl:id>GAZ:00239748</oboInOwl:id>
        <rdfs:label>KwaDengezi</rdfs:label>
    </owl:NamedIndividual>
    


    <!-- http://purl.obolibrary.org/obo/GAZ_00239749 -->

    <owl:NamedIndividual rdf:about="http://purl.obolibrary.org/obo/GAZ_00239749">
        <obo:RO_0001025 rdf:resource="http://purl.obolibrary.org/obo/GAZ_00239651"/>
        <obo:IAO_0000115>A suburb of Durban.</obo:IAO_0000115>
        <oboInOwl:hasOBONamespace>GAZ</oboInOwl:hasOBONamespace>
        <oboInOwl:id>GAZ:00239749</oboInOwl:id>
        <rdfs:label>Escombe</rdfs:label>
    </owl:NamedIndividual>
    


    <!-- http://purl.obolibrary.org/obo/GAZ_00239750 -->

    <owl:NamedIndividual rdf:about="http://purl.obolibrary.org/obo/GAZ_00239750">
        <obo:RO_0001025 rdf:resource="http://purl.obolibrary.org/obo/GAZ_00239651"/>
        <obo:IAO_0000115>A suburb of Durban.</obo:IAO_0000115>
        <oboInOwl:hasOBONamespace>GAZ</oboInOwl:hasOBONamespace>
        <oboInOwl:id>GAZ:00239750</oboInOwl:id>
        <rdfs:label>Malvern</rdfs:label>
    </owl:NamedIndividual>
    


    <!-- http://purl.obolibrary.org/obo/GAZ_00239751 -->

    <owl:NamedIndividual rdf:about="http://purl.obolibrary.org/obo/GAZ_00239751">
        <obo:RO_0001025 rdf:resource="http://purl.obolibrary.org/obo/GAZ_00239651"/>
        <obo:IAO_0000115>A suburb of Durban.</obo:IAO_0000115>
        <oboInOwl:hasOBONamespace>GAZ</oboInOwl:hasOBONamespace>
        <oboInOwl:id>GAZ:00239751</oboInOwl:id>
        <rdfs:label>Maryvale</rdfs:label>
    </owl:NamedIndividual>
    


    <!-- http://purl.obolibrary.org/obo/GAZ_00239752 -->

    <owl:NamedIndividual rdf:about="http://purl.obolibrary.org/obo/GAZ_00239752">
        <obo:RO_0001025 rdf:resource="http://purl.obolibrary.org/obo/GAZ_00239651"/>
        <obo:IAO_0000115>A suburb of Durban.</obo:IAO_0000115>
        <oboInOwl:hasOBONamespace>GAZ</oboInOwl:hasOBONamespace>
        <oboInOwl:id>GAZ:00239752</oboInOwl:id>
        <rdfs:label>Marianridge</rdfs:label>
    </owl:NamedIndividual>
    


    <!-- http://purl.obolibrary.org/obo/GAZ_00239753 -->

    <owl:NamedIndividual rdf:about="http://purl.obolibrary.org/obo/GAZ_00239753">
        <obo:RO_0001025 rdf:resource="http://purl.obolibrary.org/obo/GAZ_00239651"/>
        <obo:IAO_0000115>A suburb of Durban.</obo:IAO_0000115>
        <oboInOwl:hasOBONamespace>GAZ</oboInOwl:hasOBONamespace>
        <oboInOwl:id>GAZ:00239753</oboInOwl:id>
        <rdfs:label>Marianhill</rdfs:label>
    </owl:NamedIndividual>
    


    <!-- http://purl.obolibrary.org/obo/GAZ_00239754 -->

    <owl:NamedIndividual rdf:about="http://purl.obolibrary.org/obo/GAZ_00239754">
        <obo:RO_0001025 rdf:resource="http://purl.obolibrary.org/obo/GAZ_00239651"/>
        <obo:IAO_0000115>A suburb of Durban.</obo:IAO_0000115>
        <oboInOwl:hasOBONamespace>GAZ</oboInOwl:hasOBONamespace>
        <oboInOwl:id>GAZ:00239754</oboInOwl:id>
        <rdfs:label>Moseley</rdfs:label>
    </owl:NamedIndividual>
    


    <!-- http://purl.obolibrary.org/obo/GAZ_00239755 -->

    <owl:NamedIndividual rdf:about="http://purl.obolibrary.org/obo/GAZ_00239755">
        <obo:RO_0001025 rdf:resource="http://purl.obolibrary.org/obo/GAZ_00239651"/>
        <obo:IAO_0000115>A suburb of Durban.</obo:IAO_0000115>
        <oboInOwl:hasOBONamespace>GAZ</oboInOwl:hasOBONamespace>
        <oboInOwl:id>GAZ:00239755</oboInOwl:id>
        <rdfs:label>New Germany</rdfs:label>
    </owl:NamedIndividual>
    


    <!-- http://purl.obolibrary.org/obo/GAZ_00239756 -->

    <owl:NamedIndividual rdf:about="http://purl.obolibrary.org/obo/GAZ_00239756">
        <obo:RO_0001025 rdf:resource="http://purl.obolibrary.org/obo/GAZ_00239651"/>
        <obo:IAO_0000115>A suburb of Durban.</obo:IAO_0000115>
        <oboInOwl:hasOBONamespace>GAZ</oboInOwl:hasOBONamespace>
        <oboInOwl:id>GAZ:00239756</oboInOwl:id>
        <rdfs:label>Pinetown</rdfs:label>
    </owl:NamedIndividual>
    


    <!-- http://purl.obolibrary.org/obo/GAZ_00239757 -->

    <owl:NamedIndividual rdf:about="http://purl.obolibrary.org/obo/GAZ_00239757">
        <obo:RO_0001025 rdf:resource="http://purl.obolibrary.org/obo/GAZ_00239651"/>
        <obo:IAO_0000115>A suburb of Durban.</obo:IAO_0000115>
        <oboInOwl:hasOBONamespace>GAZ</oboInOwl:hasOBONamespace>
        <oboInOwl:id>GAZ:00239757</oboInOwl:id>
        <rdfs:label>Queensburgh</rdfs:label>
    </owl:NamedIndividual>
    


    <!-- http://purl.obolibrary.org/obo/GAZ_00239758 -->

    <owl:NamedIndividual rdf:about="http://purl.obolibrary.org/obo/GAZ_00239758">
        <obo:RO_0001025 rdf:resource="http://purl.obolibrary.org/obo/GAZ_00239651"/>
        <obo:IAO_0000115>A suburb of Durban.</obo:IAO_0000115>
        <oboInOwl:hasOBONamespace>GAZ</oboInOwl:hasOBONamespace>
        <oboInOwl:id>GAZ:00239758</oboInOwl:id>
        <rdfs:label>Reservior Hills</rdfs:label>
    </owl:NamedIndividual>
    


    <!-- http://purl.obolibrary.org/obo/GAZ_00239759 -->

    <owl:NamedIndividual rdf:about="http://purl.obolibrary.org/obo/GAZ_00239759">
        <obo:RO_0001025 rdf:resource="http://purl.obolibrary.org/obo/GAZ_00239651"/>
        <obo:IAO_0000115>A suburb of Durban.</obo:IAO_0000115>
        <oboInOwl:hasOBONamespace>GAZ</oboInOwl:hasOBONamespace>
        <oboInOwl:id>GAZ:00239759</oboInOwl:id>
        <rdfs:label>Shallcross</rdfs:label>
    </owl:NamedIndividual>
    


    <!-- http://purl.obolibrary.org/obo/GAZ_00239760 -->

    <owl:NamedIndividual rdf:about="http://purl.obolibrary.org/obo/GAZ_00239760">
        <obo:RO_0001025 rdf:resource="http://purl.obolibrary.org/obo/GAZ_00239651"/>
        <obo:IAO_0000115>A suburb of Durban.</obo:IAO_0000115>
        <oboInOwl:hasOBONamespace>GAZ</oboInOwl:hasOBONamespace>
        <oboInOwl:id>GAZ:00239760</oboInOwl:id>
        <rdfs:label>Sarnia</rdfs:label>
    </owl:NamedIndividual>
    


    <!-- http://purl.obolibrary.org/obo/GAZ_00239761 -->

    <owl:NamedIndividual rdf:about="http://purl.obolibrary.org/obo/GAZ_00239761">
        <obo:RO_0001025 rdf:resource="http://purl.obolibrary.org/obo/GAZ_00239651"/>
        <obo:IAO_0000115>A suburb of Durban.</obo:IAO_0000115>
        <oboInOwl:hasOBONamespace>GAZ</oboInOwl:hasOBONamespace>
        <oboInOwl:id>GAZ:00239761</oboInOwl:id>
        <rdfs:label>Savanna Park</rdfs:label>
    </owl:NamedIndividual>
    


    <!-- http://purl.obolibrary.org/obo/GAZ_00239762 -->

    <owl:NamedIndividual rdf:about="http://purl.obolibrary.org/obo/GAZ_00239762">
        <obo:RO_0001025 rdf:resource="http://purl.obolibrary.org/obo/GAZ_00239651"/>
        <obo:IAO_0000115>A suburb of Durban.</obo:IAO_0000115>
        <oboInOwl:hasOBONamespace>GAZ</oboInOwl:hasOBONamespace>
        <oboInOwl:id>GAZ:00239762</oboInOwl:id>
        <rdfs:label>St Wendolins</rdfs:label>
    </owl:NamedIndividual>
    


    <!-- http://purl.obolibrary.org/obo/GAZ_00239763 -->

    <owl:NamedIndividual rdf:about="http://purl.obolibrary.org/obo/GAZ_00239763">
        <obo:RO_0001025 rdf:resource="http://purl.obolibrary.org/obo/GAZ_00239651"/>
        <obo:IAO_0000115>A suburb of Durban.</obo:IAO_0000115>
        <oboInOwl:hasOBONamespace>GAZ</oboInOwl:hasOBONamespace>
        <oboInOwl:id>GAZ:00239763</oboInOwl:id>
        <rdfs:label>Shallcross</rdfs:label>
    </owl:NamedIndividual>
    


    <!-- http://purl.obolibrary.org/obo/GAZ_00239764 -->

    <owl:NamedIndividual rdf:about="http://purl.obolibrary.org/obo/GAZ_00239764">
        <obo:RO_0001025 rdf:resource="http://purl.obolibrary.org/obo/GAZ_00239651"/>
        <obo:IAO_0000115>A suburb of Durban.</obo:IAO_0000115>
        <oboInOwl:hasOBONamespace>GAZ</oboInOwl:hasOBONamespace>
        <oboInOwl:id>GAZ:00239764</oboInOwl:id>
        <rdfs:label>Thornwood</rdfs:label>
    </owl:NamedIndividual>
    


    <!-- http://purl.obolibrary.org/obo/GAZ_00239765 -->

    <owl:NamedIndividual rdf:about="http://purl.obolibrary.org/obo/GAZ_00239765">
        <obo:RO_0001025 rdf:resource="http://purl.obolibrary.org/obo/GAZ_00239651"/>
        <obo:IAO_0000115>A suburb of Durban.</obo:IAO_0000115>
        <oboInOwl:hasOBONamespace>GAZ</oboInOwl:hasOBONamespace>
        <oboInOwl:id>GAZ:00239765</oboInOwl:id>
        <rdfs:label>Welbedacht</rdfs:label>
    </owl:NamedIndividual>
    


    <!-- http://purl.obolibrary.org/obo/GAZ_00239766 -->

    <owl:NamedIndividual rdf:about="http://purl.obolibrary.org/obo/GAZ_00239766">
        <obo:RO_0001025 rdf:resource="http://purl.obolibrary.org/obo/GAZ_00239651"/>
        <obo:IAO_0000115>A suburb of Durban.</obo:IAO_0000115>
        <oboInOwl:hasOBONamespace>GAZ</oboInOwl:hasOBONamespace>
        <oboInOwl:id>GAZ:00239766</oboInOwl:id>
        <rdfs:label>Westville</rdfs:label>
    </owl:NamedIndividual>
    


    <!-- http://purl.obolibrary.org/obo/GAZ_00239767 -->

    <owl:NamedIndividual rdf:about="http://purl.obolibrary.org/obo/GAZ_00239767">
        <obo:RO_0001025 rdf:resource="http://purl.obolibrary.org/obo/GAZ_00239652"/>
        <obo:IAO_0000115>A suburb of Durban.</obo:IAO_0000115>
        <oboInOwl:hasOBONamespace>GAZ</oboInOwl:hasOBONamespace>
        <oboInOwl:id>GAZ:00239767</oboInOwl:id>
        <rdfs:label>Amanzimtoti</rdfs:label>
    </owl:NamedIndividual>
    


    <!-- http://purl.obolibrary.org/obo/GAZ_00239768 -->

    <owl:NamedIndividual rdf:about="http://purl.obolibrary.org/obo/GAZ_00239768">
        <obo:RO_0001025 rdf:resource="http://purl.obolibrary.org/obo/GAZ_00239652"/>
        <obo:IAO_0000115>A suburb of Durban.</obo:IAO_0000115>
        <oboInOwl:hasOBONamespace>GAZ</oboInOwl:hasOBONamespace>
        <oboInOwl:id>GAZ:00239768</oboInOwl:id>
        <rdfs:label>Clansthal</rdfs:label>
    </owl:NamedIndividual>
    


    <!-- http://purl.obolibrary.org/obo/GAZ_00239769 -->

    <owl:NamedIndividual rdf:about="http://purl.obolibrary.org/obo/GAZ_00239769">
        <obo:RO_0001025 rdf:resource="http://purl.obolibrary.org/obo/GAZ_00239652"/>
        <obo:IAO_0000115>A suburb of Durban.</obo:IAO_0000115>
        <oboInOwl:hasOBONamespace>GAZ</oboInOwl:hasOBONamespace>
        <oboInOwl:id>GAZ:00239769</oboInOwl:id>
        <rdfs:label>Craigieburn</rdfs:label>
    </owl:NamedIndividual>
    


    <!-- http://purl.obolibrary.org/obo/GAZ_00239770 -->

    <owl:NamedIndividual rdf:about="http://purl.obolibrary.org/obo/GAZ_00239770">
        <obo:RO_0001025 rdf:resource="http://purl.obolibrary.org/obo/GAZ_00239652"/>
        <obo:IAO_0000115>A suburb of Durban.</obo:IAO_0000115>
        <oboInOwl:hasOBONamespace>GAZ</oboInOwl:hasOBONamespace>
        <oboInOwl:id>GAZ:00239770</oboInOwl:id>
        <rdfs:label>Isipingo</rdfs:label>
    </owl:NamedIndividual>
    


    <!-- http://purl.obolibrary.org/obo/GAZ_00239771 -->

    <owl:NamedIndividual rdf:about="http://purl.obolibrary.org/obo/GAZ_00239771">
        <obo:RO_0001025 rdf:resource="http://purl.obolibrary.org/obo/GAZ_00239652"/>
        <obo:IAO_0000115>A suburb of Durban.</obo:IAO_0000115>
        <oboInOwl:hasOBONamespace>GAZ</oboInOwl:hasOBONamespace>
        <oboInOwl:id>GAZ:00239771</oboInOwl:id>
        <rdfs:label>Isipingo Beach</rdfs:label>
    </owl:NamedIndividual>
    


    <!-- http://purl.obolibrary.org/obo/GAZ_00239772 -->

    <owl:NamedIndividual rdf:about="http://purl.obolibrary.org/obo/GAZ_00239772">
        <obo:RO_0001025 rdf:resource="http://purl.obolibrary.org/obo/GAZ_00239652"/>
        <obo:IAO_0000115>A suburb of Durban.</obo:IAO_0000115>
        <oboInOwl:hasOBONamespace>GAZ</oboInOwl:hasOBONamespace>
        <oboInOwl:id>GAZ:00239772</oboInOwl:id>
        <rdfs:label>Kingsborough</rdfs:label>
    </owl:NamedIndividual>
    


    <!-- http://purl.obolibrary.org/obo/GAZ_00239773 -->

    <owl:NamedIndividual rdf:about="http://purl.obolibrary.org/obo/GAZ_00239773">
        <obo:RO_0001025 rdf:resource="http://purl.obolibrary.org/obo/GAZ_00239652"/>
        <obo:IAO_0000115>A suburb of Durban.</obo:IAO_0000115>
        <oboInOwl:hasOBONamespace>GAZ</oboInOwl:hasOBONamespace>
        <oboInOwl:id>GAZ:00239773</oboInOwl:id>
        <rdfs:label>KwaMakuta</rdfs:label>
    </owl:NamedIndividual>
    


    <!-- http://purl.obolibrary.org/obo/GAZ_00239774 -->

    <owl:NamedIndividual rdf:about="http://purl.obolibrary.org/obo/GAZ_00239774">
        <obo:RO_0001025 rdf:resource="http://purl.obolibrary.org/obo/GAZ_00239652"/>
        <obo:IAO_0000115>A suburb of Durban.</obo:IAO_0000115>
        <oboInOwl:hasOBONamespace>GAZ</oboInOwl:hasOBONamespace>
        <oboInOwl:id>GAZ:00239774</oboInOwl:id>
        <rdfs:label>Lower Illovo</rdfs:label>
    </owl:NamedIndividual>
    


    <!-- http://purl.obolibrary.org/obo/GAZ_00239775 -->

    <owl:NamedIndividual rdf:about="http://purl.obolibrary.org/obo/GAZ_00239775">
        <obo:RO_0001025 rdf:resource="http://purl.obolibrary.org/obo/GAZ_00239652"/>
        <obo:IAO_0000115>A suburb of Durban.</obo:IAO_0000115>
        <oboInOwl:hasOBONamespace>GAZ</oboInOwl:hasOBONamespace>
        <oboInOwl:id>GAZ:00239775</oboInOwl:id>
        <rdfs:label>Lovu</rdfs:label>
    </owl:NamedIndividual>
    


    <!-- http://purl.obolibrary.org/obo/GAZ_00239776 -->

    <owl:NamedIndividual rdf:about="http://purl.obolibrary.org/obo/GAZ_00239776">
        <obo:RO_0001025 rdf:resource="http://purl.obolibrary.org/obo/GAZ_00239652"/>
        <obo:IAO_0000115>A suburb of Durban.</obo:IAO_0000115>
        <oboInOwl:hasOBONamespace>GAZ</oboInOwl:hasOBONamespace>
        <oboInOwl:id>GAZ:00239776</oboInOwl:id>
        <rdfs:label>Magabeni</rdfs:label>
    </owl:NamedIndividual>
    


    <!-- http://purl.obolibrary.org/obo/GAZ_00239777 -->

    <owl:NamedIndividual rdf:about="http://purl.obolibrary.org/obo/GAZ_00239777">
        <obo:RO_0001025 rdf:resource="http://purl.obolibrary.org/obo/GAZ_00239652"/>
        <obo:IAO_0000115>A suburb of Durban.</obo:IAO_0000115>
        <oboInOwl:hasOBONamespace>GAZ</oboInOwl:hasOBONamespace>
        <oboInOwl:id>GAZ:00239777</oboInOwl:id>
        <rdfs:label>Reunion</rdfs:label>
    </owl:NamedIndividual>
    


    <!-- http://purl.obolibrary.org/obo/GAZ_00239778 -->

    <owl:NamedIndividual rdf:about="http://purl.obolibrary.org/obo/GAZ_00239778">
        <obo:RO_0001025 rdf:resource="http://purl.obolibrary.org/obo/GAZ_00239652"/>
        <obo:IAO_0000115>A suburb of Durban.</obo:IAO_0000115>
        <oboInOwl:hasOBONamespace>GAZ</oboInOwl:hasOBONamespace>
        <oboInOwl:id>GAZ:00239778</oboInOwl:id>
        <rdfs:label>Umbogintweni</rdfs:label>
    </owl:NamedIndividual>
    


    <!-- http://purl.obolibrary.org/obo/GAZ_00239779 -->

    <owl:NamedIndividual rdf:about="http://purl.obolibrary.org/obo/GAZ_00239779">
        <obo:RO_0001025 rdf:resource="http://purl.obolibrary.org/obo/GAZ_00239652"/>
        <obo:IAO_0000115>A suburb of Durban.</obo:IAO_0000115>
        <oboInOwl:hasOBONamespace>GAZ</oboInOwl:hasOBONamespace>
        <oboInOwl:id>GAZ:00239779</oboInOwl:id>
        <rdfs:label>Umkomaas</rdfs:label>
    </owl:NamedIndividual>
    


    <!-- http://purl.obolibrary.org/obo/GAZ_00239780 -->

    <owl:NamedIndividual rdf:about="http://purl.obolibrary.org/obo/GAZ_00239780">
        <obo:RO_0001025 rdf:resource="http://purl.obolibrary.org/obo/GAZ_00239652"/>
        <obo:IAO_0000115>A suburb of Durban.</obo:IAO_0000115>
        <oboInOwl:hasOBONamespace>GAZ</oboInOwl:hasOBONamespace>
        <oboInOwl:id>GAZ:00239780</oboInOwl:id>
        <rdfs:label>Warner Beach</rdfs:label>
    </owl:NamedIndividual>
    


    <!-- http://purl.obolibrary.org/obo/GAZ_00239781 -->

    <owl:NamedIndividual rdf:about="http://purl.obolibrary.org/obo/GAZ_00239781">
        <obo:RO_0001025 rdf:resource="http://purl.obolibrary.org/obo/GAZ_00239652"/>
        <obo:IAO_0000115>A suburb of Durban.</obo:IAO_0000115>
        <oboInOwl:hasOBONamespace>GAZ</oboInOwl:hasOBONamespace>
        <oboInOwl:id>GAZ:00239781</oboInOwl:id>
        <rdfs:label>Widenham</rdfs:label>
    </owl:NamedIndividual>
    


    <!-- http://purl.obolibrary.org/obo/GAZ_00239782 -->

    <owl:NamedIndividual rdf:about="http://purl.obolibrary.org/obo/GAZ_00239782">
        <obo:RO_0001025 rdf:resource="http://purl.obolibrary.org/obo/GAZ_00010007"/>
        <obo:IAO_0000115>A protected area. Located at the mouth of the Umgeni River in Durban. Established 1977.</obo:IAO_0000115>
        <oboInOwl:hasOBONamespace>GAZ</oboInOwl:hasOBONamespace>
        <oboInOwl:id>GAZ:00239782</oboInOwl:id>
        <rdfs:label>Beachwood Mangroves</rdfs:label>
    </owl:NamedIndividual>
    


    <!-- http://purl.obolibrary.org/obo/GAZ_00239783 -->

    <owl:NamedIndividual rdf:about="http://purl.obolibrary.org/obo/GAZ_00239783">
        <obo:RO_0001025 rdf:resource="http://purl.obolibrary.org/obo/GAZ_00002812"/>
        <obo:IAO_0000115>A protected area.</obo:IAO_0000115>
        <oboInOwl:hasOBONamespace>GAZ</oboInOwl:hasOBONamespace>
        <oboInOwl:id>GAZ:00239783</oboInOwl:id>
        <rdfs:label>Blinkwater Nature Reserve</rdfs:label>
    </owl:NamedIndividual>
    


    <!-- http://purl.obolibrary.org/obo/GAZ_00239784 -->

    <owl:NamedIndividual rdf:about="http://purl.obolibrary.org/obo/GAZ_00239784">
        <obo:RO_0001025 rdf:resource="http://purl.obolibrary.org/obo/GAZ_00239655"/>
        <obo:IAO_0000115>A protected area that consists of a large pan and adjacent forest and is situated in the Bluff suburb of Durban. Established 1974-10-24.</obo:IAO_0000115>
        <oboInOwl:hasOBONamespace>GAZ</oboInOwl:hasOBONamespace>
        <oboInOwl:id>GAZ:00239784</oboInOwl:id>
        <rdfs:label>Bluff Nature Reserve</rdfs:label>
    </owl:NamedIndividual>
    


    <!-- http://purl.obolibrary.org/obo/GAZ_00239785 -->

    <owl:NamedIndividual rdf:about="http://purl.obolibrary.org/obo/GAZ_00239785">
        <obo:RO_0001025 rdf:resource="http://purl.obolibrary.org/obo/GAZ_00002812"/>
        <oboInOwl:hasOBONamespace>GAZ</oboInOwl:hasOBONamespace>
        <oboInOwl:id>GAZ:00239785</oboInOwl:id>
        <rdfs:label>uKhahlamba Drakensberg Park</rdfs:label>
    </owl:NamedIndividual>
    


    <!-- http://purl.obolibrary.org/obo/GAZ_00239786 -->

    <owl:NamedIndividual rdf:about="http://purl.obolibrary.org/obo/GAZ_00239786">
        <obo:RO_0001025 rdf:resource="http://purl.obolibrary.org/obo/GAZ_00239789"/>
        <obo:IAO_0000115>A protected area.</obo:IAO_0000115>
        <oboInOwl:hasOBONamespace>GAZ</oboInOwl:hasOBONamespace>
        <oboInOwl:id>GAZ:00239786</oboInOwl:id>
        <rdfs:label>Bushman&apos;s Neck Valley</rdfs:label>
    </owl:NamedIndividual>
    


    <!-- http://purl.obolibrary.org/obo/GAZ_00239787 -->

    <owl:NamedIndividual rdf:about="http://purl.obolibrary.org/obo/GAZ_00239787">
        <obo:RO_0001025 rdf:resource="http://purl.obolibrary.org/obo/GAZ_00239785"/>
        <obo:IAO_0000115>A protected area.</obo:IAO_0000115>
        <oboInOwl:hasOBONamespace>GAZ</oboInOwl:hasOBONamespace>
        <oboInOwl:id>GAZ:00239787</oboInOwl:id>
        <rdfs:label>Cathedral Peak</rdfs:label>
    </owl:NamedIndividual>
    


    <!-- http://purl.obolibrary.org/obo/GAZ_00239788 -->

    <owl:NamedIndividual rdf:about="http://purl.obolibrary.org/obo/GAZ_00239788">
        <obo:RO_0001025 rdf:resource="http://purl.obolibrary.org/obo/GAZ_00239785"/>
        <obo:IAO_0000115>A protected area located adjacent to Himeville Village.</obo:IAO_0000115>
        <oboInOwl:hasOBONamespace>GAZ</oboInOwl:hasOBONamespace>
        <oboInOwl:id>GAZ:00239788</oboInOwl:id>
        <rdfs:label>Cobham Reserve</rdfs:label>
    </owl:NamedIndividual>
    


    <!-- http://purl.obolibrary.org/obo/GAZ_00239789 -->

    <owl:NamedIndividual rdf:about="http://purl.obolibrary.org/obo/GAZ_00239789">
        <obo:RO_0001025 rdf:resource="http://purl.obolibrary.org/obo/GAZ_00239785"/>
        <obo:IAO_0000115>The southern most part of the uKhahlamba Drakensberg Park.</obo:IAO_0000115>
        <oboInOwl:hasOBONamespace>GAZ</oboInOwl:hasOBONamespace>
        <oboInOwl:id>GAZ:00239789</oboInOwl:id>
        <rdfs:label>Garden Castle</rdfs:label>
    </owl:NamedIndividual>
    


    <!-- http://purl.obolibrary.org/obo/GAZ_00239790 -->

    <owl:NamedIndividual rdf:about="http://purl.obolibrary.org/obo/GAZ_00239790">
        <obo:RO_0001025 rdf:resource="http://purl.obolibrary.org/obo/GAZ_00239785"/>
        <obo:IAO_0000115>A protected area located in the Ukhahlamba Drakensberg Park&apos;s Central Region and is bordered by Kamberg and Lotheni to the South and Giants Castle to the North.</obo:IAO_0000115>
        <oboInOwl:hasOBONamespace>GAZ</oboInOwl:hasOBONamespace>
        <oboInOwl:id>GAZ:00239790</oboInOwl:id>
        <rdfs:label>Highmoor Nature Reserve</rdfs:label>
    </owl:NamedIndividual>
    


    <!-- http://purl.obolibrary.org/obo/GAZ_00239791 -->

    <owl:NamedIndividual rdf:about="http://purl.obolibrary.org/obo/GAZ_00239791">
        <obo:RO_0001025 rdf:resource="http://purl.obolibrary.org/obo/GAZ_00239785"/>
        <obo:IAO_0000115>A protected area.</obo:IAO_0000115>
        <oboInOwl:hasOBONamespace>GAZ</oboInOwl:hasOBONamespace>
        <oboInOwl:id>GAZ:00239791</oboInOwl:id>
        <rdfs:label>Lotheni Reserve</rdfs:label>
    </owl:NamedIndividual>
    


    <!-- http://purl.obolibrary.org/obo/GAZ_00239792 -->

    <owl:NamedIndividual rdf:about="http://purl.obolibrary.org/obo/GAZ_00239792">
        <obo:RO_0001025 rdf:resource="http://purl.obolibrary.org/obo/GAZ_00239785"/>
        <obo:IAO_0000115>A protected area.</obo:IAO_0000115>
        <oboInOwl:hasOBONamespace>GAZ</oboInOwl:hasOBONamespace>
        <oboInOwl:id>GAZ:00239792</oboInOwl:id>
        <rdfs:label>Mkhomazi Reserve</rdfs:label>
    </owl:NamedIndividual>
    


    <!-- http://purl.obolibrary.org/obo/GAZ_00239793 -->

    <owl:NamedIndividual rdf:about="http://purl.obolibrary.org/obo/GAZ_00239793">
        <obo:RO_0001025 rdf:resource="http://purl.obolibrary.org/obo/GAZ_00239785"/>
        <obo:IAO_0000115>A protected area.</obo:IAO_0000115>
        <oboInOwl:hasOBONamespace>GAZ</oboInOwl:hasOBONamespace>
        <oboInOwl:id>GAZ:00239793</oboInOwl:id>
        <rdfs:label>Monks Cowl</rdfs:label>
    </owl:NamedIndividual>
    


    <!-- http://purl.obolibrary.org/obo/GAZ_00239794 -->

    <owl:NamedIndividual rdf:about="http://purl.obolibrary.org/obo/GAZ_00239794">
        <obo:RO_0001025 rdf:resource="http://purl.obolibrary.org/obo/GAZ_00005308"/>
        <obo:IAO_0000115>A protected area.</obo:IAO_0000115>
        <oboInOwl:hasOBONamespace>GAZ</oboInOwl:hasOBONamespace>
        <oboInOwl:id>GAZ:00239794</oboInOwl:id>
        <rdfs:label>Cape Vidal State Forest</rdfs:label>
    </owl:NamedIndividual>
    


    <!-- http://purl.obolibrary.org/obo/GAZ_00239795 -->

    <owl:NamedIndividual rdf:about="http://purl.obolibrary.org/obo/GAZ_00239795">
        <obo:RO_0001025 rdf:resource="http://purl.obolibrary.org/obo/GAZ_00005308"/>
        <oboInOwl:hasOBONamespace>GAZ</oboInOwl:hasOBONamespace>
        <oboInOwl:id>GAZ:00239795</oboInOwl:id>
        <rdfs:label>Coastal Forest Reserve</rdfs:label>
    </owl:NamedIndividual>
    


    <!-- http://purl.obolibrary.org/obo/GAZ_00239796 -->

    <owl:NamedIndividual rdf:about="http://purl.obolibrary.org/obo/GAZ_00239796">
        <obo:RO_0001025 rdf:resource="http://purl.obolibrary.org/obo/GAZ_00005308"/>
        <oboInOwl:hasOBONamespace>GAZ</oboInOwl:hasOBONamespace>
        <oboInOwl:id>GAZ:00239796</oboInOwl:id>
        <rdfs:label>Eastern Shores State Forest</rdfs:label>
    </owl:NamedIndividual>
    


    <!-- http://purl.obolibrary.org/obo/GAZ_00239797 -->

    <owl:NamedIndividual rdf:about="http://purl.obolibrary.org/obo/GAZ_00239797">
        <obo:RO_0001025 rdf:resource="http://purl.obolibrary.org/obo/GAZ_00005308"/>
        <oboInOwl:hasOBONamespace>GAZ</oboInOwl:hasOBONamespace>
        <oboInOwl:id>GAZ:00239797</oboInOwl:id>
        <rdfs:label>Nyalazi State Forest</rdfs:label>
    </owl:NamedIndividual>
    


    <!-- http://purl.obolibrary.org/obo/GAZ_00239798 -->

    <owl:NamedIndividual rdf:about="http://purl.obolibrary.org/obo/GAZ_00239798">
        <obo:RO_0001025 rdf:resource="http://purl.obolibrary.org/obo/GAZ_00005308"/>
        <oboInOwl:hasOBONamespace>GAZ</oboInOwl:hasOBONamespace>
        <oboInOwl:id>GAZ:00239798</oboInOwl:id>
        <rdfs:label>Maputaland Marine Reserve</rdfs:label>
    </owl:NamedIndividual>
    


    <!-- http://purl.obolibrary.org/obo/GAZ_00239799 -->

    <owl:NamedIndividual rdf:about="http://purl.obolibrary.org/obo/GAZ_00239799">
        <obo:RO_0001025 rdf:resource="http://purl.obolibrary.org/obo/GAZ_00005308"/>
        <oboInOwl:hasOBONamespace>GAZ</oboInOwl:hasOBONamespace>
        <oboInOwl:id>GAZ:00239799</oboInOwl:id>
        <rdfs:label>Lake Sibayi Freshwater Reserve</rdfs:label>
    </owl:NamedIndividual>
    


    <!-- http://purl.obolibrary.org/obo/GAZ_00239800 -->

    <owl:NamedIndividual rdf:about="http://purl.obolibrary.org/obo/GAZ_00239800">
        <obo:RO_0001025 rdf:resource="http://purl.obolibrary.org/obo/GAZ_00005308"/>
        <oboInOwl:hasOBONamespace>GAZ</oboInOwl:hasOBONamespace>
        <oboInOwl:id>GAZ:00239800</oboInOwl:id>
        <rdfs:label>Sodwana State Forest</rdfs:label>
    </owl:NamedIndividual>
    


    <!-- http://purl.obolibrary.org/obo/GAZ_00239802 -->

    <owl:NamedIndividual rdf:about="http://purl.obolibrary.org/obo/GAZ_00239802">
        <obo:RO_0001025 rdf:resource="http://purl.obolibrary.org/obo/GAZ_00005308"/>
        <oboInOwl:hasOBONamespace>GAZ</oboInOwl:hasOBONamespace>
        <oboInOwl:id>GAZ:00239802</oboInOwl:id>
        <rdfs:label>Saint Lucia Park</rdfs:label>
    </owl:NamedIndividual>
    


    <!-- http://purl.obolibrary.org/obo/GAZ_00239803 -->

    <owl:NamedIndividual rdf:about="http://purl.obolibrary.org/obo/GAZ_00239803">
        <obo:RO_0001025 rdf:resource="http://purl.obolibrary.org/obo/GAZ_00005308"/>
        <obo:IAO_0000115>A protected area.</obo:IAO_0000115>
        <oboInOwl:hasOBONamespace>GAZ</oboInOwl:hasOBONamespace>
        <oboInOwl:id>GAZ:00239803</oboInOwl:id>
        <rdfs:label>Umkhuze Game Reserve</rdfs:label>
    </owl:NamedIndividual>
    


    <!-- http://purl.obolibrary.org/obo/GAZ_00239804 -->

    <owl:NamedIndividual rdf:about="http://purl.obolibrary.org/obo/GAZ_00239804">
        <obo:RO_0001025 rdf:resource="http://purl.obolibrary.org/obo/GAZ_00239787"/>
        <obo:IAO_0000115>A valley.</obo:IAO_0000115>
        <oboInOwl:hasOBONamespace>GAZ</oboInOwl:hasOBONamespace>
        <oboInOwl:id>GAZ:00239804</oboInOwl:id>
        <rdfs:label>Didima Valley</rdfs:label>
    </owl:NamedIndividual>
    


    <!-- http://purl.obolibrary.org/obo/GAZ_00239805 -->

    <owl:NamedIndividual rdf:about="http://purl.obolibrary.org/obo/GAZ_00239805">
        <obo:RO_0001025 rdf:resource="http://purl.obolibrary.org/obo/GAZ_00239787"/>
        <obo:IAO_0000115>A mountain.</obo:IAO_0000115>
        <oboInOwl:hasOBONamespace>GAZ</oboInOwl:hasOBONamespace>
        <oboInOwl:id>GAZ:00239805</oboInOwl:id>
        <rdfs:label>Cathedral Peak</rdfs:label>
    </owl:NamedIndividual>
    


    <!-- http://purl.obolibrary.org/obo/GAZ_00239806 -->

    <owl:NamedIndividual rdf:about="http://purl.obolibrary.org/obo/GAZ_00239806">
        <obo:RO_0001025 rdf:resource="http://purl.obolibrary.org/obo/GAZ_00005308"/>
        <obo:IAO_0000115>A protected area.</obo:IAO_0000115>
        <oboInOwl:hasOBONamespace>GAZ</oboInOwl:hasOBONamespace>
        <oboInOwl:id>GAZ:00239806</oboInOwl:id>
        <rdfs:label>Charter&apos;s Creek</rdfs:label>
    </owl:NamedIndividual>
    


    <!-- http://purl.obolibrary.org/obo/GAZ_00239807 -->

    <owl:NamedIndividual rdf:about="http://purl.obolibrary.org/obo/GAZ_00239807">
        <obo:RO_0001025 rdf:resource="http://purl.obolibrary.org/obo/GAZ_00002812"/>
        <obo:IAO_0000115>A protected area.</obo:IAO_0000115>
        <oboInOwl:hasOBONamespace>GAZ</oboInOwl:hasOBONamespace>
        <oboInOwl:id>GAZ:00239807</oboInOwl:id>
        <rdfs:label>Ncandu Nature Reserve</rdfs:label>
    </owl:NamedIndividual>
    


    <!-- http://purl.obolibrary.org/obo/GAZ_00239809 -->

    <owl:NamedIndividual rdf:about="http://purl.obolibrary.org/obo/GAZ_00239809">
        <obo:IAO_0000115>A dam. Impounds Chelmsford Dam Reservoir.</obo:IAO_0000115>
        <oboInOwl:hasOBONamespace>GAZ</oboInOwl:hasOBONamespace>
        <oboInOwl:id>GAZ:00239809</oboInOwl:id>
        <rdfs:label>Chelmsford Dam</rdfs:label>
    </owl:NamedIndividual>
    


    <!-- http://purl.obolibrary.org/obo/GAZ_00239810 -->

    <owl:NamedIndividual rdf:about="http://purl.obolibrary.org/obo/GAZ_00239810">
        <obo:IAO_0000115>A reservoir. Impounded by Chelmsford Dam.</obo:IAO_0000115>
        <oboInOwl:hasOBONamespace>GAZ</oboInOwl:hasOBONamespace>
        <oboInOwl:id>GAZ:00239810</oboInOwl:id>
        <rdfs:label>Chelmsford Dam Reservoir</rdfs:label>
    </owl:NamedIndividual>
    


    <!-- http://purl.obolibrary.org/obo/GAZ_00239811 -->

    <owl:NamedIndividual rdf:about="http://purl.obolibrary.org/obo/GAZ_00239811">
        <obo:RO_0001025 rdf:resource="http://purl.obolibrary.org/obo/GAZ_00239626"/>
        <obo:IAO_0000115>A protected area.</obo:IAO_0000115>
        <oboInOwl:hasOBONamespace>GAZ</oboInOwl:hasOBONamespace>
        <oboInOwl:id>GAZ:00239811</oboInOwl:id>
        <rdfs:label>Entumeni Forest</rdfs:label>
    </owl:NamedIndividual>
    


    <!-- http://purl.obolibrary.org/obo/GAZ_00239812 -->

    <owl:NamedIndividual rdf:about="http://purl.obolibrary.org/obo/GAZ_00239812">
        <obo:RO_0001025 rdf:resource="http://purl.obolibrary.org/obo/GAZ_00002812"/>
        <obo:IAO_0000115>A protected area.</obo:IAO_0000115>
        <oboInOwl:hasOBONamespace>GAZ</oboInOwl:hasOBONamespace>
        <oboInOwl:id>GAZ:00239812</oboInOwl:id>
        <rdfs:label>Enseleni Nature Reserve</rdfs:label>
    </owl:NamedIndividual>
    


    <!-- http://purl.obolibrary.org/obo/GAZ_00239815 -->

    <owl:NamedIndividual rdf:about="http://purl.obolibrary.org/obo/GAZ_00239815">
        <obo:RO_0001025 rdf:resource="http://purl.obolibrary.org/obo/GAZ_00239816"/>
        <obo:IAO_0000115>A protected area. An island.</obo:IAO_0000115>
        <oboInOwl:hasOBONamespace>GAZ</oboInOwl:hasOBONamespace>
        <oboInOwl:id>GAZ:00239815</oboInOwl:id>
        <rdfs:label>Fanie&apos;s Island</rdfs:label>
    </owl:NamedIndividual>
    


    <!-- http://purl.obolibrary.org/obo/GAZ_00239816 -->

    <owl:NamedIndividual rdf:about="http://purl.obolibrary.org/obo/GAZ_00239816">
        <obo:RO_0001025 rdf:resource="http://purl.obolibrary.org/obo/GAZ_00005308"/>
        <obo:IAO_0000115>A tidal estuary.</obo:IAO_0000115>
        <oboInOwl:hasOBONamespace>GAZ</oboInOwl:hasOBONamespace>
        <oboInOwl:id>GAZ:00239816</oboInOwl:id>
        <rdfs:label>Lake Saint Lucia</rdfs:label>
    </owl:NamedIndividual>
    


    <!-- http://purl.obolibrary.org/obo/GAZ_00239817 -->

    <owl:NamedIndividual rdf:about="http://purl.obolibrary.org/obo/GAZ_00239817">
        <obo:RO_0001025 rdf:resource="http://purl.obolibrary.org/obo/GAZ_00239785"/>
        <obo:IAO_0000115>A protected area located in the Central Berg region of the Ukhahlamba Drakensberg Park.</obo:IAO_0000115>
        <oboInOwl:hasOBONamespace>GAZ</oboInOwl:hasOBONamespace>
        <oboInOwl:id>GAZ:00239817</oboInOwl:id>
        <rdfs:label>Giant&apos;s Castle Game Reserve</rdfs:label>
    </owl:NamedIndividual>
    


    <!-- http://purl.obolibrary.org/obo/GAZ_00239818 -->

    <owl:NamedIndividual rdf:about="http://purl.obolibrary.org/obo/GAZ_00239818">
        <obo:RO_0001025 rdf:resource="http://purl.obolibrary.org/obo/GAZ_00002812"/>
        <obo:IAO_0000115>A protected area. Located on the south bank of the Thukela River, the reserve is 6 km from the river mouth on the KwaZulu-Natal North Coast.</obo:IAO_0000115>
        <oboInOwl:hasOBONamespace>GAZ</oboInOwl:hasOBONamespace>
        <oboInOwl:id>GAZ:00239818</oboInOwl:id>
        <rdfs:label>Harold Johnson Nature Reserve</rdfs:label>
    </owl:NamedIndividual>
    


    <!-- http://purl.obolibrary.org/obo/GAZ_00239822 -->

    <owl:NamedIndividual rdf:about="http://purl.obolibrary.org/obo/GAZ_00239822">
        <obo:RO_0001025 rdf:resource="http://purl.obolibrary.org/obo/GAZ_00002812"/>
        <obo:IAO_0000115>A protected area.</obo:IAO_0000115>
        <oboInOwl:hasOBONamespace>GAZ</oboInOwl:hasOBONamespace>
        <oboInOwl:id>GAZ:00239822</oboInOwl:id>
        <rdfs:label>Imfolozi Game Reserve</rdfs:label>
    </owl:NamedIndividual>
    


    <!-- http://purl.obolibrary.org/obo/GAZ_00239823 -->

    <owl:NamedIndividual rdf:about="http://purl.obolibrary.org/obo/GAZ_00239823">
        <obo:RO_0001025 rdf:resource="http://purl.obolibrary.org/obo/GAZ_00002812"/>
        <obo:IAO_0000115>A protected area.</obo:IAO_0000115>
        <oboInOwl:hasOBONamespace>GAZ</oboInOwl:hasOBONamespace>
        <oboInOwl:id>GAZ:00239823</oboInOwl:id>
        <rdfs:label>Impendle Nature Reserve</rdfs:label>
    </owl:NamedIndividual>
    


    <!-- http://purl.obolibrary.org/obo/GAZ_00239824 -->

    <owl:NamedIndividual rdf:about="http://purl.obolibrary.org/obo/GAZ_00239824">
        <obo:RO_0001025 rdf:resource="http://purl.obolibrary.org/obo/GAZ_00239701"/>
        <obo:IAO_0000115>A protected area. Established 1963.</obo:IAO_0000115>
        <oboInOwl:hasOBONamespace>GAZ</oboInOwl:hasOBONamespace>
        <oboInOwl:id>GAZ:00239824</oboInOwl:id>
        <rdfs:label>Kenneth Stainbank Nature Reserve</rdfs:label>
    </owl:NamedIndividual>
    


    <!-- http://purl.obolibrary.org/obo/GAZ_00239825 -->

    <owl:NamedIndividual rdf:about="http://purl.obolibrary.org/obo/GAZ_00239825">
        <obo:RO_0001025 rdf:resource="http://purl.obolibrary.org/obo/GAZ_00005308"/>
        <obo:IAO_0000115>A protected area.</obo:IAO_0000115>
        <oboInOwl:hasOBONamespace>GAZ</oboInOwl:hasOBONamespace>
        <oboInOwl:id>GAZ:00239825</oboInOwl:id>
        <rdfs:label>Kosi Bay Nature Reserve</rdfs:label>
    </owl:NamedIndividual>
    


    <!-- http://purl.obolibrary.org/obo/GAZ_00239826 -->

    <owl:NamedIndividual rdf:about="http://purl.obolibrary.org/obo/GAZ_00239826">
        <obo:RO_0001025 rdf:resource="http://purl.obolibrary.org/obo/GAZ_00002812"/>
        <obo:IAO_0000115>A protected area located 20 km south of Margate.</obo:IAO_0000115>
        <oboInOwl:hasOBONamespace>GAZ</oboInOwl:hasOBONamespace>
        <oboInOwl:id>GAZ:00239826</oboInOwl:id>
        <rdfs:label>Mpenjati Nature Reserve</rdfs:label>
    </owl:NamedIndividual>
    


    <!-- http://purl.obolibrary.org/obo/GAZ_00239827 -->

    <owl:NamedIndividual rdf:about="http://purl.obolibrary.org/obo/GAZ_00239827">
        <obo:RO_0001025 rdf:resource="http://purl.obolibrary.org/obo/GAZ_00002812"/>
        <obo:IAO_0000115>A protected area.</obo:IAO_0000115>
        <oboInOwl:hasOBONamespace>GAZ</oboInOwl:hasOBONamespace>
        <oboInOwl:id>GAZ:00239827</oboInOwl:id>
        <rdfs:label>Wagendrift Nature Reserve</rdfs:label>
    </owl:NamedIndividual>
    


    <!-- http://purl.obolibrary.org/obo/GAZ_00239828 -->

    <owl:NamedIndividual rdf:about="http://purl.obolibrary.org/obo/GAZ_00239828">
        <obo:RO_0001025 rdf:resource="http://purl.obolibrary.org/obo/GAZ_00239827"/>
        <obo:IAO_0000115>A dam. Impounds Wagendrift Dam Reservoir.</obo:IAO_0000115>
        <oboInOwl:hasOBONamespace>GAZ</oboInOwl:hasOBONamespace>
        <oboInOwl:id>GAZ:00239828</oboInOwl:id>
        <rdfs:label>Wagendrift Dam</rdfs:label>
    </owl:NamedIndividual>
    


    <!-- http://purl.obolibrary.org/obo/GAZ_00239829 -->

    <owl:NamedIndividual rdf:about="http://purl.obolibrary.org/obo/GAZ_00239829">
        <obo:RO_0001025 rdf:resource="http://purl.obolibrary.org/obo/GAZ_00239827"/>
        <obo:IAO_0000115>A reservoir impounded by Wagendrift Dam.</obo:IAO_0000115>
        <oboInOwl:hasOBONamespace>GAZ</oboInOwl:hasOBONamespace>
        <oboInOwl:id>GAZ:00239829</oboInOwl:id>
        <rdfs:label>Wagendrift Dam Reservoir</rdfs:label>
    </owl:NamedIndividual>
    


    <!-- http://purl.obolibrary.org/obo/GAZ_00239830 -->

    <owl:NamedIndividual rdf:about="http://purl.obolibrary.org/obo/GAZ_00239830">
        <obo:RO_0001025 rdf:resource="http://purl.obolibrary.org/obo/GAZ_00239827"/>
        <obo:IAO_0000115>A protected area.</obo:IAO_0000115>
        <oboInOwl:hasOBONamespace>GAZ</oboInOwl:hasOBONamespace>
        <oboInOwl:id>GAZ:00239830</oboInOwl:id>
        <rdfs:label>Moor Park Reserve</rdfs:label>
    </owl:NamedIndividual>
    


    <!-- http://purl.obolibrary.org/obo/GAZ_00239832 -->

    <owl:NamedIndividual rdf:about="http://purl.obolibrary.org/obo/GAZ_00239832">
        <obo:RO_0001025 rdf:resource="http://purl.obolibrary.org/obo/GAZ_00002812"/>
        <obo:IAO_0000115>A protected area. It covers the crown and south-western slopes of the ridge which lies above the Mhlatuze and Thukela rivers at a height of between 1100 and 1300 m above sea level.</obo:IAO_0000115>
        <oboInOwl:hasOBONamespace>GAZ</oboInOwl:hasOBONamespace>
        <oboInOwl:id>GAZ:00239832</oboInOwl:id>
        <rdfs:label>Nkandla Forest</rdfs:label>
    </owl:NamedIndividual>
    


    <!-- http://purl.obolibrary.org/obo/GAZ_00239833 -->

    <owl:NamedIndividual rdf:about="http://purl.obolibrary.org/obo/GAZ_00239833">
        <obo:RO_0001025 rdf:resource="http://purl.obolibrary.org/obo/GAZ_00002812"/>
        <obo:IAO_0000115>A protected area. Established 1968.</obo:IAO_0000115>
        <oboInOwl:hasOBONamespace>GAZ</oboInOwl:hasOBONamespace>
        <oboInOwl:id>GAZ:00239833</oboInOwl:id>
        <rdfs:label>North Park Nature Reserve</rdfs:label>
    </owl:NamedIndividual>
    


    <!-- http://purl.obolibrary.org/obo/GAZ_00239835 -->

    <owl:NamedIndividual rdf:about="http://purl.obolibrary.org/obo/GAZ_00239835">
        <obo:RO_0001025 rdf:resource="http://purl.obolibrary.org/obo/GAZ_00002812"/>
        <obo:IAO_0000115>A protected area.</obo:IAO_0000115>
        <oboInOwl:hasOBONamespace>GAZ</oboInOwl:hasOBONamespace>
        <oboInOwl:id>GAZ:00239835</oboInOwl:id>
        <rdfs:label>Ongoye Forest</rdfs:label>
    </owl:NamedIndividual>
    


    <!-- http://purl.obolibrary.org/obo/GAZ_00239836 -->

    <owl:NamedIndividual rdf:about="http://purl.obolibrary.org/obo/GAZ_00239836">
        <obo:RO_0001025 rdf:resource="http://purl.obolibrary.org/obo/GAZ_00002812"/>
        <obo:IAO_0000115>A protected area. Located on the southern banks of the White Mfolozi river. Established 1991.</obo:IAO_0000115>
        <oboInOwl:hasOBONamespace>GAZ</oboInOwl:hasOBONamespace>
        <oboInOwl:id>GAZ:00239836</oboInOwl:id>
        <rdfs:label>Ophathe Game Reserve</rdfs:label>
    </owl:NamedIndividual>
    


    <!-- http://purl.obolibrary.org/obo/GAZ_00239837 -->

    <owl:NamedIndividual rdf:about="http://purl.obolibrary.org/obo/GAZ_00239837">
        <obo:RO_0001025 rdf:resource="http://purl.obolibrary.org/obo/GAZ_00005308"/>
        <obo:IAO_0000115>A protected area. Located west of the Maputoland Marine Reserve, east of the Mkuzi river and swamps, and south of Sodwana Bay National Park and Mbazwana town.</obo:IAO_0000115>
        <oboInOwl:hasOBONamespace>GAZ</oboInOwl:hasOBONamespace>
        <oboInOwl:id>GAZ:00239837</oboInOwl:id>
        <rdfs:label>Ozabeni Reserve</rdfs:label>
    </owl:NamedIndividual>
    


    <!-- http://purl.obolibrary.org/obo/GAZ_00239838 -->

    <owl:NamedIndividual rdf:about="http://purl.obolibrary.org/obo/GAZ_00239838">
        <obo:RO_0001025 rdf:resource="http://purl.obolibrary.org/obo/GAZ_00239837"/>
        <obo:IAO_0000115>A lake.</obo:IAO_0000115>
        <oboInOwl:hasOBONamespace>GAZ</oboInOwl:hasOBONamespace>
        <oboInOwl:id>GAZ:00239838</oboInOwl:id>
        <rdfs:label>Lake Neshi</rdfs:label>
    </owl:NamedIndividual>
    


    <!-- http://purl.obolibrary.org/obo/GAZ_00239839 -->

    <owl:NamedIndividual rdf:about="http://purl.obolibrary.org/obo/GAZ_00239839">
        <obo:RO_0001025 rdf:resource="http://purl.obolibrary.org/obo/GAZ_00239837"/>
        <obo:IAO_0000115>A lake.</obo:IAO_0000115>
        <oboInOwl:hasOBONamespace>GAZ</oboInOwl:hasOBONamespace>
        <oboInOwl:id>GAZ:00239839</oboInOwl:id>
        <rdfs:label>Lake Mozi</rdfs:label>
    </owl:NamedIndividual>
    


    <!-- http://purl.obolibrary.org/obo/GAZ_00239840 -->

    <owl:NamedIndividual rdf:about="http://purl.obolibrary.org/obo/GAZ_00239840">
        <obo:RO_0001025 rdf:resource="http://purl.obolibrary.org/obo/GAZ_00239837"/>
        <obo:IAO_0000115>A lake.</obo:IAO_0000115>
        <oboInOwl:hasOBONamespace>GAZ</oboInOwl:hasOBONamespace>
        <oboInOwl:id>GAZ:00239840</oboInOwl:id>
        <rdfs:label>Lake Yengweni</rdfs:label>
    </owl:NamedIndividual>
    


    <!-- http://purl.obolibrary.org/obo/GAZ_00239841 -->

    <owl:NamedIndividual rdf:about="http://purl.obolibrary.org/obo/GAZ_00239841">
        <obo:RO_0001025 rdf:resource="http://purl.obolibrary.org/obo/GAZ_00239837"/>
        <obo:IAO_0000115>A lake.</obo:IAO_0000115>
        <oboInOwl:hasOBONamespace>GAZ</oboInOwl:hasOBONamespace>
        <oboInOwl:id>GAZ:00239841</oboInOwl:id>
        <rdfs:label>Lake Mdlanzi</rdfs:label>
    </owl:NamedIndividual>
    


    <!-- http://purl.obolibrary.org/obo/GAZ_00239842 -->

    <owl:NamedIndividual rdf:about="http://purl.obolibrary.org/obo/GAZ_00239842">
        <obo:RO_0001025 rdf:resource="http://purl.obolibrary.org/obo/GAZ_00239837"/>
        <obo:IAO_0000115>A lake.</obo:IAO_0000115>
        <oboInOwl:hasOBONamespace>GAZ</oboInOwl:hasOBONamespace>
        <oboInOwl:id>GAZ:00239842</oboInOwl:id>
        <rdfs:label>Lake Mpanza</rdfs:label>
    </owl:NamedIndividual>
    


    <!-- http://purl.obolibrary.org/obo/GAZ_00239843 -->

    <owl:NamedIndividual rdf:about="http://purl.obolibrary.org/obo/GAZ_00239843">
        <obo:RO_0001025 rdf:resource="http://purl.obolibrary.org/obo/GAZ_00239837"/>
        <obo:IAO_0000115>A lake.</obo:IAO_0000115>
        <oboInOwl:hasOBONamespace>GAZ</oboInOwl:hasOBONamespace>
        <oboInOwl:id>GAZ:00239843</oboInOwl:id>
        <rdfs:label>Lake Ntshangwe</rdfs:label>
    </owl:NamedIndividual>
    


    <!-- http://purl.obolibrary.org/obo/GAZ_00239844 -->

    <owl:NamedIndividual rdf:about="http://purl.obolibrary.org/obo/GAZ_00239844">
        <obo:RO_0001025 rdf:resource="http://purl.obolibrary.org/obo/GAZ_00239837"/>
        <obo:IAO_0000115>A lake.</obo:IAO_0000115>
        <oboInOwl:hasOBONamespace>GAZ</oboInOwl:hasOBONamespace>
        <oboInOwl:id>GAZ:00239844</oboInOwl:id>
        <rdfs:label>Lake Bikibiki</rdfs:label>
    </owl:NamedIndividual>
    


    <!-- http://purl.obolibrary.org/obo/GAZ_00239845 -->

    <owl:NamedIndividual rdf:about="http://purl.obolibrary.org/obo/GAZ_00239845">
        <obo:RO_0001025 rdf:resource="http://purl.obolibrary.org/obo/GAZ_00239837"/>
        <obo:IAO_0000115>A lake.</obo:IAO_0000115>
        <oboInOwl:hasOBONamespace>GAZ</oboInOwl:hasOBONamespace>
        <oboInOwl:id>GAZ:00239845</oboInOwl:id>
        <rdfs:label>Lake Mfula</rdfs:label>
    </owl:NamedIndividual>
    


    <!-- http://purl.obolibrary.org/obo/GAZ_00239846 -->

    <owl:NamedIndividual rdf:about="http://purl.obolibrary.org/obo/GAZ_00239846">
        <obo:RO_0001025 rdf:resource="http://purl.obolibrary.org/obo/GAZ_00239837"/>
        <obo:IAO_0000115>A lake.</obo:IAO_0000115>
        <oboInOwl:hasOBONamespace>GAZ</oboInOwl:hasOBONamespace>
        <oboInOwl:id>GAZ:00239846</oboInOwl:id>
        <rdfs:label>Lake Ndlebeni</rdfs:label>
    </owl:NamedIndividual>
    


    <!-- http://purl.obolibrary.org/obo/GAZ_00239847 -->

    <owl:NamedIndividual rdf:about="http://purl.obolibrary.org/obo/GAZ_00239847">
        <obo:IAO_0000115>A protected area. Established 1894-06-13.</obo:IAO_0000115>
        <oboInOwl:hasOBONamespace>GAZ</oboInOwl:hasOBONamespace>
        <oboInOwl:id>GAZ:00239847</oboInOwl:id>
        <rdfs:label>Phongolop Nature Reserve</rdfs:label>
    </owl:NamedIndividual>
    


    <!-- http://purl.obolibrary.org/obo/GAZ_00239848 -->

    <owl:NamedIndividual rdf:about="http://purl.obolibrary.org/obo/GAZ_00239848">
        <obo:RO_0001025 rdf:resource="http://purl.obolibrary.org/obo/GAZ_00239847"/>
        <obo:IAO_0000115>A dam. Constructed 1973.</obo:IAO_0000115>
        <oboInOwl:hasOBONamespace>GAZ</oboInOwl:hasOBONamespace>
        <oboInOwl:id>GAZ:00239848</oboInOwl:id>
        <rdfs:label>Phongolopoort Dam</rdfs:label>
    </owl:NamedIndividual>
    


    <!-- http://purl.obolibrary.org/obo/GAZ_00239849 -->

    <owl:NamedIndividual rdf:about="http://purl.obolibrary.org/obo/GAZ_00239849">
        <obo:RO_0001025 rdf:resource="http://purl.obolibrary.org/obo/GAZ_00008041"/>
        <obo:IAO_0000115>A protected area located he northern slopes of Pietermaritzburg.</obo:IAO_0000115>
        <oboInOwl:hasOBONamespace>GAZ</oboInOwl:hasOBONamespace>
        <oboInOwl:id>GAZ:00239849</oboInOwl:id>
        <rdfs:label>Queen Elizabeth Park Nature Reserve</rdfs:label>
    </owl:NamedIndividual>
    


    <!-- http://purl.obolibrary.org/obo/GAZ_00239850 -->

    <owl:NamedIndividual rdf:about="http://purl.obolibrary.org/obo/GAZ_00239850">
        <obo:RO_0001025 rdf:resource="http://purl.obolibrary.org/obo/GAZ_00002812"/>
        <obo:IAO_0000115>A protected area located between Uvongo and Margate. Established 1962.</obo:IAO_0000115>
        <oboInOwl:hasOBONamespace>GAZ</oboInOwl:hasOBONamespace>
        <oboInOwl:id>GAZ:00239850</oboInOwl:id>
        <rdfs:label>Skyline Nature Reserve</rdfs:label>
    </owl:NamedIndividual>
    


    <!-- http://purl.obolibrary.org/obo/GAZ_00239851 -->

    <owl:NamedIndividual rdf:about="http://purl.obolibrary.org/obo/GAZ_00239851">
        <obo:RO_0001025 rdf:resource="http://purl.obolibrary.org/obo/GAZ_00002812"/>
        <obo:IAO_0000115>A protected area.</obo:IAO_0000115>
        <oboInOwl:hasOBONamespace>GAZ</oboInOwl:hasOBONamespace>
        <oboInOwl:id>GAZ:00239851</oboInOwl:id>
        <rdfs:label>Tembe Elephant Park</rdfs:label>
    </owl:NamedIndividual>
    


    <!-- http://purl.obolibrary.org/obo/GAZ_00239852 -->

    <owl:NamedIndividual rdf:about="http://purl.obolibrary.org/obo/GAZ_00239852">
        <obo:RO_0001025 rdf:resource="http://purl.obolibrary.org/obo/GAZ_00239739"/>
        <obo:IAO_0000115>A river in KwaZulu-Natal, South Africa, which empties into the Indian Ocean just north of Umhlanga, KwaZulu-Natal, north of Durban.</obo:IAO_0000115>
        <oboInOwl:hasOBONamespace>GAZ</oboInOwl:hasOBONamespace>
        <oboInOwl:id>GAZ:00239852</oboInOwl:id>
        <rdfs:label>Umhlanga River</rdfs:label>
    </owl:NamedIndividual>
    


    <!-- http://purl.obolibrary.org/obo/GAZ_00239853 -->

    <owl:NamedIndividual rdf:about="http://purl.obolibrary.org/obo/GAZ_00239853">
        <obo:RO_0001025 rdf:resource="http://purl.obolibrary.org/obo/GAZ_00239739"/>
        <obo:IAO_0000115>A protected area.</obo:IAO_0000115>
        <oboInOwl:hasOBONamespace>GAZ</oboInOwl:hasOBONamespace>
        <oboInOwl:id>GAZ:00239853</oboInOwl:id>
        <rdfs:label>Umhlanga Lagoon Nature Reserve</rdfs:label>
    </owl:NamedIndividual>
    


    <!-- http://purl.obolibrary.org/obo/GAZ_00239854 -->

    <owl:NamedIndividual rdf:about="http://purl.obolibrary.org/obo/GAZ_00239854">
        <obo:RO_0001025 rdf:resource="http://purl.obolibrary.org/obo/GAZ_00239852"/>
        <obo:RO_0001025 rdf:resource="http://purl.obolibrary.org/obo/GAZ_00239853"/>
        <obo:IAO_0000115>A lagoon.</obo:IAO_0000115>
        <oboInOwl:hasOBONamespace>GAZ</oboInOwl:hasOBONamespace>
        <oboInOwl:id>GAZ:00239854</oboInOwl:id>
        <rdfs:label>Umhlanga Lagoon</rdfs:label>
    </owl:NamedIndividual>
    


    <!-- http://purl.obolibrary.org/obo/GAZ_00239856 -->

    <owl:NamedIndividual rdf:about="http://purl.obolibrary.org/obo/GAZ_00239856">
        <obo:RO_0001025 rdf:resource="http://purl.obolibrary.org/obo/GAZ_00075905"/>
        <obo:IAO_0000115>A protected area.</obo:IAO_0000115>
        <oboInOwl:hasOBONamespace>GAZ</oboInOwl:hasOBONamespace>
        <oboInOwl:id>GAZ:00239856</oboInOwl:id>
        <rdfs:label>Vryheid Hill Nature Reserve</rdfs:label>
    </owl:NamedIndividual>
    


    <!-- http://purl.obolibrary.org/obo/GAZ_00239857 -->

    <owl:NamedIndividual rdf:about="http://purl.obolibrary.org/obo/GAZ_00239857">
        <obo:RO_0001025 rdf:resource="http://purl.obolibrary.org/obo/GAZ_00075418"/>
        <obo:IAO_0000115>A protected area located in the Waterberg in Limpopo Province in northern South Africa.</obo:IAO_0000115>
        <oboInOwl:hasOBONamespace>GAZ</oboInOwl:hasOBONamespace>
        <oboInOwl:id>GAZ:00239857</oboInOwl:id>
        <rdfs:label>Entabeni Game Reserve</rdfs:label>
    </owl:NamedIndividual>
    


    <!-- http://purl.obolibrary.org/obo/GAZ_00239858 -->

    <owl:NamedIndividual rdf:about="http://purl.obolibrary.org/obo/GAZ_00239858">
        <rdf:type rdf:resource="http://purl.obolibrary.org/obo/ENVO_00000100"/>
        <obo:RO_0001025 rdf:resource="http://purl.obolibrary.org/obo/GAZ_00002809"/>
        <obo:IAO_0000115>A gorge located in the far North of the Kruger National Park. It forms the boundary between the Kruger National Park to the South and the Makuleke Concession to the North.</obo:IAO_0000115>
        <oboInOwl:hasOBONamespace>GAZ</oboInOwl:hasOBONamespace>
        <oboInOwl:id>GAZ:00239858</oboInOwl:id>
        <rdfs:label>Lanner Gorge</rdfs:label>
    </owl:NamedIndividual>
    


    <!-- http://purl.obolibrary.org/obo/GAZ_00239861 -->

    <owl:NamedIndividual rdf:about="http://purl.obolibrary.org/obo/GAZ_00239861">
        <obo:RO_0001025 rdf:resource="http://purl.obolibrary.org/obo/GAZ_00032882"/>
        <obo:IAO_0000115>A reservoir. Located at the village of ha-mutoti and ha-Budeli just about few km from Thohoyandou in the district of Vhembe in Limpopo province. Cosntructed 2004.</obo:IAO_0000115>
        <oboInOwl:hasOBONamespace>GAZ</oboInOwl:hasOBONamespace>
        <oboInOwl:id>GAZ:00239861</oboInOwl:id>
        <rdfs:label>Nandoni Dam</rdfs:label>
    </owl:NamedIndividual>
    


    <!-- http://purl.obolibrary.org/obo/GAZ_00239862 -->

    <owl:NamedIndividual rdf:about="http://purl.obolibrary.org/obo/GAZ_00239862">
        <obo:RO_0001025 rdf:resource="http://purl.obolibrary.org/obo/GAZ_00032881"/>
        <obo:IAO_0000115>A protected area, lying on a seasonally-inundated floodplain and located near Naboomspruit in the Limpopo Province of South Africa. A Ramsar Site.</obo:IAO_0000115>
        <oboInOwl:hasOBONamespace>GAZ</oboInOwl:hasOBONamespace>
        <oboInOwl:id>GAZ:00239862</oboInOwl:id>
        <rdfs:label>Nylsvley Nature Reserve</rdfs:label>
    </owl:NamedIndividual>
    


    <!-- http://purl.obolibrary.org/obo/GAZ_00239863 -->

    <owl:NamedIndividual rdf:about="http://purl.obolibrary.org/obo/GAZ_00239863">
        <obo:RO_0001025 rdf:resource="http://purl.obolibrary.org/obo/GAZ_00032883"/>
        <obo:IAO_0000115>A protected area.</obo:IAO_0000115>
        <oboInOwl:hasOBONamespace>GAZ</oboInOwl:hasOBONamespace>
        <oboInOwl:id>GAZ:00239863</oboInOwl:id>
        <rdfs:label>Tzaneen Dam Provincial Park</rdfs:label>
    </owl:NamedIndividual>
    


    <!-- http://purl.obolibrary.org/obo/GAZ_00239864 -->

    <owl:NamedIndividual rdf:about="http://purl.obolibrary.org/obo/GAZ_00239864">
        <obo:RO_0001025 rdf:resource="http://purl.obolibrary.org/obo/GAZ_00032883"/>
        <obo:IAO_0000115>A protected area.</obo:IAO_0000115>
        <oboInOwl:hasOBONamespace>GAZ</oboInOwl:hasOBONamespace>
        <oboInOwl:id>GAZ:00239864</oboInOwl:id>
        <rdfs:label>Man&apos;Ombe Provincial Park</rdfs:label>
    </owl:NamedIndividual>
    


    <!-- http://purl.obolibrary.org/obo/GAZ_00239865 -->

    <owl:NamedIndividual rdf:about="http://purl.obolibrary.org/obo/GAZ_00239865">
        <obo:RO_0001025 rdf:resource="http://purl.obolibrary.org/obo/GAZ_00032882"/>
        <obo:IAO_0000115>A protected area.</obo:IAO_0000115>
        <oboInOwl:hasOBONamespace>GAZ</oboInOwl:hasOBONamespace>
        <oboInOwl:id>GAZ:00239865</oboInOwl:id>
        <rdfs:label>Nwanedi Provincial Park</rdfs:label>
    </owl:NamedIndividual>
    


    <!-- http://purl.obolibrary.org/obo/GAZ_00239866 -->

    <owl:NamedIndividual rdf:about="http://purl.obolibrary.org/obo/GAZ_00239866">
        <obo:RO_0001025 rdf:resource="http://purl.obolibrary.org/obo/GAZ_00032883"/>
        <obo:IAO_0000115>A protected area.</obo:IAO_0000115>
        <oboInOwl:hasOBONamespace>GAZ</oboInOwl:hasOBONamespace>
        <oboInOwl:id>GAZ:00239866</oboInOwl:id>
        <rdfs:label>Letaba Ranch Provincial Park</rdfs:label>
    </owl:NamedIndividual>
    


    <!-- http://purl.obolibrary.org/obo/GAZ_00239867 -->

    <owl:NamedIndividual rdf:about="http://purl.obolibrary.org/obo/GAZ_00239867">
        <obo:RO_0001025 rdf:resource="http://purl.obolibrary.org/obo/GAZ_00032883"/>
        <obo:IAO_0000115>A protected area.</obo:IAO_0000115>
        <oboInOwl:hasOBONamespace>GAZ</oboInOwl:hasOBONamespace>
        <oboInOwl:id>GAZ:00239867</oboInOwl:id>
        <rdfs:label>Lekgalameetse Provincial Park</rdfs:label>
    </owl:NamedIndividual>
    


    <!-- http://purl.obolibrary.org/obo/GAZ_00239868 -->

    <owl:NamedIndividual rdf:about="http://purl.obolibrary.org/obo/GAZ_00239868">
        <obo:RO_0001025 rdf:resource="http://purl.obolibrary.org/obo/GAZ_00032881"/>
        <obo:IAO_0000115>A protected area.</obo:IAO_0000115>
        <oboInOwl:hasOBONamespace>GAZ</oboInOwl:hasOBONamespace>
        <oboInOwl:id>GAZ:00239868</oboInOwl:id>
        <rdfs:label>Atherstone Nature Reserve</rdfs:label>
    </owl:NamedIndividual>
    


    <!-- http://purl.obolibrary.org/obo/GAZ_00239869 -->

    <owl:NamedIndividual rdf:about="http://purl.obolibrary.org/obo/GAZ_00239869">
        <obo:RO_0001025 rdf:resource="http://purl.obolibrary.org/obo/GAZ_00032884"/>
        <obo:IAO_0000115>A protected area.</obo:IAO_0000115>
        <oboInOwl:hasOBONamespace>GAZ</oboInOwl:hasOBONamespace>
        <oboInOwl:id>GAZ:00239869</oboInOwl:id>
        <rdfs:label>Balule Nature Reserve</rdfs:label>
    </owl:NamedIndividual>
    


    <!-- http://purl.obolibrary.org/obo/GAZ_00239870 -->

    <owl:NamedIndividual rdf:about="http://purl.obolibrary.org/obo/GAZ_00239870">
        <obo:RO_0001025 rdf:resource="http://purl.obolibrary.org/obo/GAZ_00076239"/>
        <obo:IAO_0000115>A protected area.</obo:IAO_0000115>
        <oboInOwl:hasOBONamespace>GAZ</oboInOwl:hasOBONamespace>
        <oboInOwl:id>GAZ:00239870</oboInOwl:id>
        <rdfs:label>Blouberg Nature Reserve</rdfs:label>
    </owl:NamedIndividual>
    


    <!-- http://purl.obolibrary.org/obo/GAZ_00239871 -->

    <owl:NamedIndividual rdf:about="http://purl.obolibrary.org/obo/GAZ_00239871">
        <obo:RO_0001025 rdf:resource="http://purl.obolibrary.org/obo/GAZ_00032881"/>
        <obo:IAO_0000115>A protected area.</obo:IAO_0000115>
        <oboInOwl:hasOBONamespace>GAZ</oboInOwl:hasOBONamespace>
        <oboInOwl:id>GAZ:00239871</oboInOwl:id>
        <rdfs:label>D&apos;nyala Nature Reserve</rdfs:label>
    </owl:NamedIndividual>
    


    <!-- http://purl.obolibrary.org/obo/GAZ_00239872 -->

    <owl:NamedIndividual rdf:about="http://purl.obolibrary.org/obo/GAZ_00239872">
        <obo:RO_0001025 rdf:resource="http://purl.obolibrary.org/obo/GAZ_00032881"/>
        <obo:IAO_0000115>A protected area.</obo:IAO_0000115>
        <oboInOwl:hasOBONamespace>GAZ</oboInOwl:hasOBONamespace>
        <oboInOwl:id>GAZ:00239872</oboInOwl:id>
        <rdfs:label>Doorndraai Nature Reserve</rdfs:label>
    </owl:NamedIndividual>
    


    <!-- http://purl.obolibrary.org/obo/GAZ_00239873 -->

    <owl:NamedIndividual rdf:about="http://purl.obolibrary.org/obo/GAZ_00239873">
        <obo:RO_0001025 rdf:resource="http://purl.obolibrary.org/obo/GAZ_00032883"/>
        <obo:IAO_0000115>A protected area.</obo:IAO_0000115>
        <oboInOwl:hasOBONamespace>GAZ</oboInOwl:hasOBONamespace>
        <oboInOwl:id>GAZ:00239873</oboInOwl:id>
        <rdfs:label>Hans Merensky Wilderness</rdfs:label>
    </owl:NamedIndividual>
    


    <!-- http://purl.obolibrary.org/obo/GAZ_00239874 -->

    <owl:NamedIndividual rdf:about="http://purl.obolibrary.org/obo/GAZ_00239874">
        <obo:RO_0001025 rdf:resource="http://purl.obolibrary.org/obo/GAZ_00032883"/>
        <obo:IAO_0000115>A protected area.</obo:IAO_0000115>
        <oboInOwl:hasOBONamespace>GAZ</oboInOwl:hasOBONamespace>
        <oboInOwl:id>GAZ:00239874</oboInOwl:id>
        <rdfs:label>Lekgalameetse Reserve</rdfs:label>
    </owl:NamedIndividual>
    


    <!-- http://purl.obolibrary.org/obo/GAZ_00239875 -->

    <owl:NamedIndividual rdf:about="http://purl.obolibrary.org/obo/GAZ_00239875">
        <obo:RO_0001025 rdf:resource="http://purl.obolibrary.org/obo/GAZ_00032881"/>
        <obo:IAO_0000115>A protected area.</obo:IAO_0000115>
        <oboInOwl:hasOBONamespace>GAZ</oboInOwl:hasOBONamespace>
        <oboInOwl:id>GAZ:00239875</oboInOwl:id>
        <rdfs:label>Mabalingwe Game Reserve</rdfs:label>
    </owl:NamedIndividual>
    


    <!-- http://purl.obolibrary.org/obo/GAZ_00239876 -->

    <owl:NamedIndividual rdf:about="http://purl.obolibrary.org/obo/GAZ_00239876">
        <obo:RO_0001025 rdf:resource="http://purl.obolibrary.org/obo/GAZ_00032883"/>
        <obo:IAO_0000115>A protected area.</obo:IAO_0000115>
        <oboInOwl:hasOBONamespace>GAZ</oboInOwl:hasOBONamespace>
        <oboInOwl:id>GAZ:00239876</oboInOwl:id>
        <rdfs:label>Makalali Private Game Reserve</rdfs:label>
    </owl:NamedIndividual>
    


    <!-- http://purl.obolibrary.org/obo/GAZ_00239877 -->

    <owl:NamedIndividual rdf:about="http://purl.obolibrary.org/obo/GAZ_00239877">
        <obo:RO_0001025 rdf:resource="http://purl.obolibrary.org/obo/GAZ_00032882"/>
        <obo:IAO_0000115>A protected area.</obo:IAO_0000115>
        <oboInOwl:hasOBONamespace>GAZ</oboInOwl:hasOBONamespace>
        <oboInOwl:id>GAZ:00239877</oboInOwl:id>
        <rdfs:label>Makuya Nature Reserve</rdfs:label>
    </owl:NamedIndividual>
    


    <!-- http://purl.obolibrary.org/obo/GAZ_00239878 -->

    <owl:NamedIndividual rdf:about="http://purl.obolibrary.org/obo/GAZ_00239878">
        <obo:RO_0001025 rdf:resource="http://purl.obolibrary.org/obo/GAZ_00032882"/>
        <obo:IAO_0000115>A protected area.</obo:IAO_0000115>
        <oboInOwl:hasOBONamespace>GAZ</oboInOwl:hasOBONamespace>
        <oboInOwl:id>GAZ:00239878</oboInOwl:id>
        <rdfs:label>Manavhela Ben Lavin Nature Reserve</rdfs:label>
    </owl:NamedIndividual>
    


    <!-- http://purl.obolibrary.org/obo/GAZ_00239879 -->

    <owl:NamedIndividual rdf:about="http://purl.obolibrary.org/obo/GAZ_00239879">
        <obo:RO_0001025 rdf:resource="http://purl.obolibrary.org/obo/GAZ_00032881"/>
        <obo:IAO_0000115>A protected area.</obo:IAO_0000115>
        <oboInOwl:hasOBONamespace>GAZ</oboInOwl:hasOBONamespace>
        <oboInOwl:id>GAZ:00239879</oboInOwl:id>
        <rdfs:label>Masebe Nature Reserve</rdfs:label>
    </owl:NamedIndividual>
    


    <!-- http://purl.obolibrary.org/obo/GAZ_00239880 -->

    <owl:NamedIndividual rdf:about="http://purl.obolibrary.org/obo/GAZ_00239880">
        <obo:RO_0001025 rdf:resource="http://purl.obolibrary.org/obo/GAZ_00032883"/>
        <obo:IAO_0000115>A protected area.</obo:IAO_0000115>
        <oboInOwl:hasOBONamespace>GAZ</oboInOwl:hasOBONamespace>
        <oboInOwl:id>GAZ:00239880</oboInOwl:id>
        <rdfs:label>Modjadji Nature Reserve</rdfs:label>
    </owl:NamedIndividual>
    


    <!-- http://purl.obolibrary.org/obo/GAZ_00239881 -->

    <owl:NamedIndividual rdf:about="http://purl.obolibrary.org/obo/GAZ_00239881">
        <obo:RO_0001025 rdf:resource="http://purl.obolibrary.org/obo/GAZ_00032882"/>
        <obo:IAO_0000115>A protected area.</obo:IAO_0000115>
        <oboInOwl:hasOBONamespace>GAZ</oboInOwl:hasOBONamespace>
        <oboInOwl:id>GAZ:00239881</oboInOwl:id>
        <rdfs:label>Musina Nature Reserve</rdfs:label>
    </owl:NamedIndividual>
    


    <!-- http://purl.obolibrary.org/obo/GAZ_00239882 -->

    <owl:NamedIndividual rdf:about="http://purl.obolibrary.org/obo/GAZ_00239882">
        <obo:RO_0001025 rdf:resource="http://purl.obolibrary.org/obo/GAZ_00032884"/>
        <obo:IAO_0000115>A protected area.</obo:IAO_0000115>
        <oboInOwl:hasOBONamespace>GAZ</oboInOwl:hasOBONamespace>
        <oboInOwl:id>GAZ:00239882</oboInOwl:id>
        <rdfs:label>Percy Fyfe Conservancy</rdfs:label>
    </owl:NamedIndividual>
    


    <!-- http://purl.obolibrary.org/obo/GAZ_00239883 -->

    <owl:NamedIndividual rdf:about="http://purl.obolibrary.org/obo/GAZ_00239883">
        <obo:RO_0001025 rdf:resource="http://purl.obolibrary.org/obo/GAZ_00032881"/>
        <obo:IAO_0000115>A protected area in Limpopo Province.</obo:IAO_0000115>
        <oboInOwl:hasOBONamespace>GAZ</oboInOwl:hasOBONamespace>
        <oboInOwl:id>GAZ:00239883</oboInOwl:id>
        <rdfs:label>Rust De Winter Reserve</rdfs:label>
    </owl:NamedIndividual>
    


    <!-- http://purl.obolibrary.org/obo/GAZ_00239885 -->

    <owl:NamedIndividual rdf:about="http://purl.obolibrary.org/obo/GAZ_00239885">
        <obo:RO_0001025 rdf:resource="http://purl.obolibrary.org/obo/GAZ_00032883"/>
        <obo:IAO_0000115>A protected area.</obo:IAO_0000115>
        <oboInOwl:hasOBONamespace>GAZ</oboInOwl:hasOBONamespace>
        <oboInOwl:id>GAZ:00239885</oboInOwl:id>
        <rdfs:label>Selati Game Reserve</rdfs:label>
    </owl:NamedIndividual>
    


    <!-- http://purl.obolibrary.org/obo/GAZ_00239886 -->

    <owl:NamedIndividual rdf:about="http://purl.obolibrary.org/obo/GAZ_00239886">
        <obo:RO_0001025 rdf:resource="http://purl.obolibrary.org/obo/GAZ_00032883"/>
        <obo:IAO_0000115>A protected area that lies to the north of the Sabi Sand Game Reserve on the western edge of Kruger National Park.</obo:IAO_0000115>
        <oboInOwl:hasOBONamespace>GAZ</oboInOwl:hasOBONamespace>
        <oboInOwl:id>GAZ:00239886</oboInOwl:id>
        <rdfs:label>Timbavati Nature Reserve</rdfs:label>
    </owl:NamedIndividual>
    


    <!-- http://purl.obolibrary.org/obo/GAZ_00239887 -->

    <owl:NamedIndividual rdf:about="http://purl.obolibrary.org/obo/GAZ_00239887">
        <obo:RO_0001025 rdf:resource="http://purl.obolibrary.org/obo/GAZ_00032882"/>
        <obo:IAO_0000115>A protected area.</obo:IAO_0000115>
        <oboInOwl:hasOBONamespace>GAZ</oboInOwl:hasOBONamespace>
        <oboInOwl:id>GAZ:00239887</oboInOwl:id>
        <rdfs:label>Venetia Limpopo Nature Reserve</rdfs:label>
    </owl:NamedIndividual>
    


    <!-- http://purl.obolibrary.org/obo/GAZ_00239888 -->

    <owl:NamedIndividual rdf:about="http://purl.obolibrary.org/obo/GAZ_00239888">
        <obo:RO_0001025 rdf:resource="http://purl.obolibrary.org/obo/GAZ_00032881"/>
        <obo:IAO_0000115>A protected area.</obo:IAO_0000115>
        <oboInOwl:hasOBONamespace>GAZ</oboInOwl:hasOBONamespace>
        <oboInOwl:id>GAZ:00239888</oboInOwl:id>
        <rdfs:label>Welgevonden Private Game Reserve</rdfs:label>
    </owl:NamedIndividual>
    


    <!-- http://purl.obolibrary.org/obo/GAZ_00239889 -->

    <owl:NamedIndividual rdf:about="http://purl.obolibrary.org/obo/GAZ_00239889">
        <obo:RO_0001025 rdf:resource="http://purl.obolibrary.org/obo/GAZ_00032881"/>
        <obo:IAO_0000115>A protected area. Located 115 km north of Mokopane, with the Mogalakwena River and Glen Alpine Dam forming the eastern border.</obo:IAO_0000115>
        <oboInOwl:hasOBONamespace>GAZ</oboInOwl:hasOBONamespace>
        <oboInOwl:id>GAZ:00239889</oboInOwl:id>
        <rdfs:label>Wonderkop</rdfs:label>
    </owl:NamedIndividual>
    


    <!-- http://purl.obolibrary.org/obo/GAZ_00239891 -->

    <owl:NamedIndividual rdf:about="http://purl.obolibrary.org/obo/GAZ_00239891">
        <obo:IAO_0000115>A dam on the Olifants River, near Groblersdal, Mpumalanga, South Africa. Constructed 1939.</obo:IAO_0000115>
        <oboInOwl:hasOBONamespace>GAZ</oboInOwl:hasOBONamespace>
        <oboInOwl:id>GAZ:00239891</oboInOwl:id>
        <rdfs:label>Loskop Dam</rdfs:label>
    </owl:NamedIndividual>
    


    <!-- http://purl.obolibrary.org/obo/GAZ_00239892 -->

    <owl:NamedIndividual rdf:about="http://purl.obolibrary.org/obo/GAZ_00239892">
        <obo:IAO_0000115>A dam.</obo:IAO_0000115>
        <oboInOwl:hasOBONamespace>GAZ</oboInOwl:hasOBONamespace>
        <oboInOwl:id>GAZ:00239892</oboInOwl:id>
        <rdfs:label>Witbank Dam</rdfs:label>
    </owl:NamedIndividual>
    


    <!-- http://purl.obolibrary.org/obo/GAZ_00239894 -->

    <owl:NamedIndividual rdf:about="http://purl.obolibrary.org/obo/GAZ_00239894">
        <obo:RO_0001025 rdf:resource="http://purl.obolibrary.org/obo/GAZ_00239883"/>
        <obo:IAO_0000115>A reservoir.</obo:IAO_0000115>
        <oboInOwl:hasOBONamespace>GAZ</oboInOwl:hasOBONamespace>
        <oboInOwl:id>GAZ:00239894</oboInOwl:id>
        <rdfs:label>Rust de Winter Dam</rdfs:label>
    </owl:NamedIndividual>
    


    <!-- http://purl.obolibrary.org/obo/GAZ_00239895 -->

    <owl:NamedIndividual rdf:about="http://purl.obolibrary.org/obo/GAZ_00239895">
        <obo:RO_0001025 rdf:resource="http://purl.obolibrary.org/obo/GAZ_00076032"/>
        <obo:IAO_0000115>A reservoir.</obo:IAO_0000115>
        <oboInOwl:hasOBONamespace>GAZ</oboInOwl:hasOBONamespace>
        <oboInOwl:id>GAZ:00239895</oboInOwl:id>
        <rdfs:label>Schuinsdraai Dam</rdfs:label>
    </owl:NamedIndividual>
    


    <!-- http://purl.obolibrary.org/obo/GAZ_00239898 -->

    <owl:NamedIndividual rdf:about="http://purl.obolibrary.org/obo/GAZ_00239898">
        <obo:RO_0001025 rdf:resource="http://purl.obolibrary.org/obo/GAZ_00076243"/>
        <obo:IAO_0000115>A protected area.</obo:IAO_0000115>
        <oboInOwl:hasOBONamespace>GAZ</oboInOwl:hasOBONamespace>
        <oboInOwl:id>GAZ:00239898</oboInOwl:id>
        <rdfs:label>Idube Safari Lodge</rdfs:label>
    </owl:NamedIndividual>
    


    <!-- http://purl.obolibrary.org/obo/GAZ_00239899 -->

    <owl:NamedIndividual rdf:about="http://purl.obolibrary.org/obo/GAZ_00239899">
        <obo:RO_0001025 rdf:resource="http://purl.obolibrary.org/obo/GAZ_00076243"/>
        <obo:IAO_0000115>A protected area.</obo:IAO_0000115>
        <oboInOwl:hasOBONamespace>GAZ</oboInOwl:hasOBONamespace>
        <oboInOwl:id>GAZ:00239899</oboInOwl:id>
        <rdfs:label>Chitwa Chitwa Game Lodge</rdfs:label>
    </owl:NamedIndividual>
    


    <!-- http://purl.obolibrary.org/obo/GAZ_00239900 -->

    <owl:NamedIndividual rdf:about="http://purl.obolibrary.org/obo/GAZ_00239900">
        <obo:RO_0001025 rdf:resource="http://purl.obolibrary.org/obo/GAZ_00076243"/>
        <obo:IAO_0000115>A protected area.</obo:IAO_0000115>
        <oboInOwl:hasOBONamespace>GAZ</oboInOwl:hasOBONamespace>
        <oboInOwl:id>GAZ:00239900</oboInOwl:id>
        <rdfs:label>Djuma Game Reserve</rdfs:label>
    </owl:NamedIndividual>
    


    <!-- http://purl.obolibrary.org/obo/GAZ_00239901 -->

    <owl:NamedIndividual rdf:about="http://purl.obolibrary.org/obo/GAZ_00239901">
        <obo:RO_0001025 rdf:resource="http://purl.obolibrary.org/obo/GAZ_00076243"/>
        <obo:IAO_0000115>A protected area.</obo:IAO_0000115>
        <oboInOwl:hasOBONamespace>GAZ</oboInOwl:hasOBONamespace>
        <oboInOwl:id>GAZ:00239901</oboInOwl:id>
        <rdfs:label>Exeter Game Lodge</rdfs:label>
    </owl:NamedIndividual>
    


    <!-- http://purl.obolibrary.org/obo/GAZ_00239902 -->

    <owl:NamedIndividual rdf:about="http://purl.obolibrary.org/obo/GAZ_00239902">
        <obo:RO_0001025 rdf:resource="http://purl.obolibrary.org/obo/GAZ_00076243"/>
        <obo:IAO_0000115>A protected area.</obo:IAO_0000115>
        <oboInOwl:hasOBONamespace>GAZ</oboInOwl:hasOBONamespace>
        <oboInOwl:id>GAZ:00239902</oboInOwl:id>
        <rdfs:label>Inyati Private Game Reserve</rdfs:label>
    </owl:NamedIndividual>
    


    <!-- http://purl.obolibrary.org/obo/GAZ_00239903 -->

    <owl:NamedIndividual rdf:about="http://purl.obolibrary.org/obo/GAZ_00239903">
        <obo:RO_0001025 rdf:resource="http://purl.obolibrary.org/obo/GAZ_00076243"/>
        <obo:IAO_0000115>A protected area.</obo:IAO_0000115>
        <oboInOwl:hasOBONamespace>GAZ</oboInOwl:hasOBONamespace>
        <oboInOwl:id>GAZ:00239903</oboInOwl:id>
        <rdfs:label>Leopard Hills Private Game Reserve</rdfs:label>
    </owl:NamedIndividual>
    


    <!-- http://purl.obolibrary.org/obo/GAZ_00239904 -->

    <owl:NamedIndividual rdf:about="http://purl.obolibrary.org/obo/GAZ_00239904">
        <obo:RO_0001025 rdf:resource="http://purl.obolibrary.org/obo/GAZ_00076243"/>
        <obo:IAO_0000115>A protected area.</obo:IAO_0000115>
        <oboInOwl:hasOBONamespace>GAZ</oboInOwl:hasOBONamespace>
        <oboInOwl:id>GAZ:00239904</oboInOwl:id>
        <rdfs:label>Lion Sands Private Game Reserve</rdfs:label>
    </owl:NamedIndividual>
    


    <!-- http://purl.obolibrary.org/obo/GAZ_00239905 -->

    <owl:NamedIndividual rdf:about="http://purl.obolibrary.org/obo/GAZ_00239905">
        <obo:RO_0001025 rdf:resource="http://purl.obolibrary.org/obo/GAZ_00076243"/>
        <obo:IAO_0000115>A protected area.</obo:IAO_0000115>
        <oboInOwl:hasOBONamespace>GAZ</oboInOwl:hasOBONamespace>
        <oboInOwl:id>GAZ:00239905</oboInOwl:id>
        <rdfs:label>Savanna Private Game Reserve</rdfs:label>
    </owl:NamedIndividual>
    


    <!-- http://purl.obolibrary.org/obo/GAZ_00239906 -->

    <owl:NamedIndividual rdf:about="http://purl.obolibrary.org/obo/GAZ_00239906">
        <obo:RO_0001025 rdf:resource="http://purl.obolibrary.org/obo/GAZ_00076243"/>
        <obo:IAO_0000115>A protected area.</obo:IAO_0000115>
        <oboInOwl:hasOBONamespace>GAZ</oboInOwl:hasOBONamespace>
        <oboInOwl:id>GAZ:00239906</oboInOwl:id>
        <rdfs:label>Ulusaba Game Lodge</rdfs:label>
    </owl:NamedIndividual>
    


    <!-- http://purl.obolibrary.org/obo/GAZ_00239907 -->

    <owl:NamedIndividual rdf:about="http://purl.obolibrary.org/obo/GAZ_00239907">
        <obo:RO_0001025 rdf:resource="http://purl.obolibrary.org/obo/GAZ_00002816"/>
        <obo:IAO_0000115>A protected area in Mpumalanga, South Africa.</obo:IAO_0000115>
        <oboInOwl:hasOBONamespace>GAZ</oboInOwl:hasOBONamespace>
        <oboInOwl:id>GAZ:00239907</oboInOwl:id>
        <rdfs:label>Blyde River Canyon Nature Reserve</rdfs:label>
    </owl:NamedIndividual>
    


    <!-- http://purl.obolibrary.org/obo/GAZ_00239908 -->

    <owl:NamedIndividual rdf:about="http://purl.obolibrary.org/obo/GAZ_00239908">
        <obo:RO_0001025 rdf:resource="http://purl.obolibrary.org/obo/GAZ_00076246"/>
        <obo:IAO_0000115>A reservoir.</obo:IAO_0000115>
        <oboInOwl:hasOBONamespace>GAZ</oboInOwl:hasOBONamespace>
        <oboInOwl:id>GAZ:00239908</oboInOwl:id>
        <rdfs:label>Loskop Dam Reservoir</rdfs:label>
    </owl:NamedIndividual>
    


    <!-- http://purl.obolibrary.org/obo/GAZ_00239909 -->

    <owl:NamedIndividual rdf:about="http://purl.obolibrary.org/obo/GAZ_00239909">
        <obo:RO_0001025 rdf:resource="http://purl.obolibrary.org/obo/GAZ_00002816"/>
        <obo:IAO_0000115>A protected area.</obo:IAO_0000115>
        <oboInOwl:hasOBONamespace>GAZ</oboInOwl:hasOBONamespace>
        <oboInOwl:id>GAZ:00239909</oboInOwl:id>
        <rdfs:label>Mabusa Nature Reserve</rdfs:label>
    </owl:NamedIndividual>
    


    <!-- http://purl.obolibrary.org/obo/GAZ_00239910 -->

    <owl:NamedIndividual rdf:about="http://purl.obolibrary.org/obo/GAZ_00239910">
        <obo:RO_0001025 rdf:resource="http://purl.obolibrary.org/obo/GAZ_00002816"/>
        <obo:IAO_0000115>A protected area.</obo:IAO_0000115>
        <oboInOwl:hasOBONamespace>GAZ</oboInOwl:hasOBONamespace>
        <oboInOwl:id>GAZ:00239910</oboInOwl:id>
        <rdfs:label>Mahushe Shongwe Reserve</rdfs:label>
    </owl:NamedIndividual>
    


    <!-- http://purl.obolibrary.org/obo/GAZ_00239911 -->

    <owl:NamedIndividual rdf:about="http://purl.obolibrary.org/obo/GAZ_00239911">
        <obo:RO_0001025 rdf:resource="http://purl.obolibrary.org/obo/GAZ_00002816"/>
        <obo:IAO_0000115>A protected area.</obo:IAO_0000115>
        <oboInOwl:hasOBONamespace>GAZ</oboInOwl:hasOBONamespace>
        <oboInOwl:id>GAZ:00239911</oboInOwl:id>
        <rdfs:label>Mkhombo Nature Reserve</rdfs:label>
    </owl:NamedIndividual>
    


    <!-- http://purl.obolibrary.org/obo/GAZ_00239913 -->

    <owl:NamedIndividual rdf:about="http://purl.obolibrary.org/obo/GAZ_00239913">
        <obo:IAO_0000115>A dam. Impounds Ohrigstad Dam Reservoir.</obo:IAO_0000115>
        <oboInOwl:hasOBONamespace>GAZ</oboInOwl:hasOBONamespace>
        <oboInOwl:id>GAZ:00239913</oboInOwl:id>
        <rdfs:label>Ohrigstad Dam</rdfs:label>
    </owl:NamedIndividual>
    


    <!-- http://purl.obolibrary.org/obo/GAZ_00239914 -->

    <owl:NamedIndividual rdf:about="http://purl.obolibrary.org/obo/GAZ_00239914">
        <obo:IAO_0000115>A reservoir impounded by Ohrigstad Dam. Constructed 1955.</obo:IAO_0000115>
        <oboInOwl:hasOBONamespace>GAZ</oboInOwl:hasOBONamespace>
        <oboInOwl:id>GAZ:00239914</oboInOwl:id>
        <rdfs:label>Ohrigstad Dam Reservoir</rdfs:label>
    </owl:NamedIndividual>
    


    <!-- http://purl.obolibrary.org/obo/GAZ_00239915 -->

    <owl:NamedIndividual rdf:about="http://purl.obolibrary.org/obo/GAZ_00239915">
        <obo:RO_0001025 rdf:resource="http://purl.obolibrary.org/obo/GAZ_00002816"/>
        <obo:IAO_0000115>A protected area.</obo:IAO_0000115>
        <oboInOwl:hasOBONamespace>GAZ</oboInOwl:hasOBONamespace>
        <oboInOwl:id>GAZ:00239915</oboInOwl:id>
        <rdfs:label>SS Skosana Nature Reserve</rdfs:label>
    </owl:NamedIndividual>
    


    <!-- http://purl.obolibrary.org/obo/GAZ_00239916 -->

    <owl:NamedIndividual rdf:about="http://purl.obolibrary.org/obo/GAZ_00239916">
        <obo:RO_0001025 rdf:resource="http://purl.obolibrary.org/obo/GAZ_00002816"/>
        <obo:IAO_0000115>A protected area.</obo:IAO_0000115>
        <oboInOwl:hasOBONamespace>GAZ</oboInOwl:hasOBONamespace>
        <oboInOwl:id>GAZ:00239916</oboInOwl:id>
        <rdfs:label>Verloren Valei Nature Reserve</rdfs:label>
    </owl:NamedIndividual>
    


    <!-- http://purl.obolibrary.org/obo/GAZ_00239917 -->

    <owl:NamedIndividual rdf:about="http://purl.obolibrary.org/obo/GAZ_00239917">
        <obo:RO_0001025 rdf:resource="http://purl.obolibrary.org/obo/GAZ_00032874"/>
        <obo:IAO_0000115>A protected area. Located between Delareyville and Sannieshof. A Ramsar Site.</obo:IAO_0000115>
        <oboInOwl:hasOBONamespace>GAZ</oboInOwl:hasOBONamespace>
        <oboInOwl:id>GAZ:00239917</oboInOwl:id>
        <rdfs:label>Barberspan Bird Sanctuary</rdfs:label>
    </owl:NamedIndividual>
    


    <!-- http://purl.obolibrary.org/obo/GAZ_00239918 -->

    <owl:NamedIndividual rdf:about="http://purl.obolibrary.org/obo/GAZ_00239918">
        <obo:RO_0001025 rdf:resource="http://purl.obolibrary.org/obo/GAZ_00032877"/>
        <obo:IAO_0000115>A protected area.</obo:IAO_0000115>
        <oboInOwl:hasOBONamespace>GAZ</oboInOwl:hasOBONamespace>
        <oboInOwl:id>GAZ:00239918</oboInOwl:id>
        <rdfs:label>Borakalalo National Park</rdfs:label>
    </owl:NamedIndividual>
    


    <!-- http://purl.obolibrary.org/obo/GAZ_00239919 -->

    <owl:NamedIndividual rdf:about="http://purl.obolibrary.org/obo/GAZ_00239919">
        <obo:RO_0001025 rdf:resource="http://purl.obolibrary.org/obo/GAZ_00032875"/>
    </owl:NamedIndividual>
    


    <!-- http://purl.obolibrary.org/obo/GAZ_00239920 -->

    <owl:NamedIndividual rdf:about="http://purl.obolibrary.org/obo/GAZ_00239920">
        <obo:RO_0001025 rdf:resource="http://purl.obolibrary.org/obo/GAZ_00032874"/>
        <obo:IAO_0000115>A protected area in North West Province.</obo:IAO_0000115>
        <oboInOwl:hasOBONamespace>GAZ</oboInOwl:hasOBONamespace>
        <oboInOwl:id>GAZ:00239920</oboInOwl:id>
        <rdfs:label>Botsalano Game Reserve</rdfs:label>
    </owl:NamedIndividual>
    


    <!-- http://purl.obolibrary.org/obo/GAZ_00239921 -->

    <owl:NamedIndividual rdf:about="http://purl.obolibrary.org/obo/GAZ_00239921">
        <obo:RO_0001025 rdf:resource="http://purl.obolibrary.org/obo/GAZ_00032877"/>
        <obo:IAO_0000115>A protected area.</obo:IAO_0000115>
        <oboInOwl:hasOBONamespace>GAZ</oboInOwl:hasOBONamespace>
        <oboInOwl:id>GAZ:00239921</oboInOwl:id>
        <rdfs:label>Kgaswane Mountain Reserve</rdfs:label>
    </owl:NamedIndividual>
    


    <!-- http://purl.obolibrary.org/obo/GAZ_00239922 -->

    <owl:NamedIndividual rdf:about="http://purl.obolibrary.org/obo/GAZ_00239922">
        <obo:RO_0001025 rdf:resource="http://purl.obolibrary.org/obo/GAZ_00032874"/>
        <obo:IAO_0000115>A protected area.</obo:IAO_0000115>
        <oboInOwl:hasOBONamespace>GAZ</oboInOwl:hasOBONamespace>
        <oboInOwl:id>GAZ:00239922</oboInOwl:id>
        <rdfs:label>Mafikeng Game Reserve</rdfs:label>
    </owl:NamedIndividual>
    


    <!-- http://purl.obolibrary.org/obo/GAZ_00239923 -->

    <owl:NamedIndividual rdf:about="http://purl.obolibrary.org/obo/GAZ_00239923">
        <obo:RO_0001025 rdf:resource="http://purl.obolibrary.org/obo/GAZ_00032874"/>
        <obo:IAO_0000115>A protected area.</obo:IAO_0000115>
        <oboInOwl:hasOBONamespace>GAZ</oboInOwl:hasOBONamespace>
        <oboInOwl:id>GAZ:00239923</oboInOwl:id>
        <rdfs:label>Molemane Eye Nature Reserve</rdfs:label>
    </owl:NamedIndividual>
    


    <!-- http://purl.obolibrary.org/obo/GAZ_00239925 -->

    <owl:NamedIndividual rdf:about="http://purl.obolibrary.org/obo/GAZ_00239925">
        <obo:RO_0001025 rdf:resource="http://purl.obolibrary.org/obo/GAZ_00032877"/>
        <oboInOwl:hasOBONamespace>GAZ</oboInOwl:hasOBONamespace>
        <oboInOwl:id>GAZ:00239925</oboInOwl:id>
        <rdfs:label>Vaalkop Dam Nature Reserve</rdfs:label>
    </owl:NamedIndividual>
    


    <!-- http://purl.obolibrary.org/obo/GAZ_00239926 -->

    <owl:NamedIndividual rdf:about="http://purl.obolibrary.org/obo/GAZ_00239926">
        <obo:RO_0001025 rdf:resource="http://purl.obolibrary.org/obo/GAZ_00032875"/>
        <obo:IAO_0000115>A protected area.</obo:IAO_0000115>
        <oboInOwl:hasOBONamespace>GAZ</oboInOwl:hasOBONamespace>
        <oboInOwl:id>GAZ:00239926</oboInOwl:id>
        <rdfs:label>Wolwespruit Dam Reserve</rdfs:label>
    </owl:NamedIndividual>
    


    <!-- http://purl.obolibrary.org/obo/GAZ_00239927 -->

    <owl:NamedIndividual rdf:about="http://purl.obolibrary.org/obo/GAZ_00239927">
        <obo:RO_0001025 rdf:resource="http://purl.obolibrary.org/obo/GAZ_00239917"/>
        <obo:IAO_0000115>A shallow, perennial, alkaline lake.</obo:IAO_0000115>
        <oboInOwl:hasOBONamespace>GAZ</oboInOwl:hasOBONamespace>
        <oboInOwl:id>GAZ:00239927</oboInOwl:id>
        <rdfs:label>Barberspan</rdfs:label>
    </owl:NamedIndividual>
    


    <!-- http://purl.obolibrary.org/obo/GAZ_00239928 -->

    <owl:NamedIndividual rdf:about="http://purl.obolibrary.org/obo/GAZ_00239928">
        <obo:RO_0001025 rdf:resource="http://purl.obolibrary.org/obo/GAZ_00239925"/>
        <obo:IAO_0000115>A reservoir.</obo:IAO_0000115>
        <oboInOwl:hasOBONamespace>GAZ</oboInOwl:hasOBONamespace>
        <oboInOwl:id>GAZ:00239928</oboInOwl:id>
        <rdfs:label>Vaalkop Dam Reservoir</rdfs:label>
    </owl:NamedIndividual>
    


    <!-- http://purl.obolibrary.org/obo/GAZ_00239930 -->

    <owl:NamedIndividual rdf:about="http://purl.obolibrary.org/obo/GAZ_00239930">
        <obo:RO_0001025 rdf:resource="http://purl.obolibrary.org/obo/GAZ_00032876"/>
        <obo:IAO_0000115>A protected area.</obo:IAO_0000115>
        <oboInOwl:hasOBONamespace>GAZ</oboInOwl:hasOBONamespace>
        <oboInOwl:id>GAZ:00239930</oboInOwl:id>
        <rdfs:label>Leon Taljaard Nature Reserve</rdfs:label>
    </owl:NamedIndividual>
    


    <!-- http://purl.obolibrary.org/obo/GAZ_00239935 -->

    <owl:NamedIndividual rdf:about="http://purl.obolibrary.org/obo/GAZ_00239935">
        <obo:RO_0001025 rdf:resource="http://purl.obolibrary.org/obo/GAZ_00032877"/>
        <obo:IAO_0000115>A reservoir.</obo:IAO_0000115>
        <oboInOwl:hasOBONamespace>GAZ</oboInOwl:hasOBONamespace>
        <oboInOwl:id>GAZ:00239935</oboInOwl:id>
        <rdfs:label>Molatedi Dam Reservoir</rdfs:label>
    </owl:NamedIndividual>
    


    <!-- http://purl.obolibrary.org/obo/GAZ_00239936 -->

    <owl:NamedIndividual rdf:about="http://purl.obolibrary.org/obo/GAZ_00239936">
        <obo:RO_0001025 rdf:resource="http://purl.obolibrary.org/obo/GAZ_00076259"/>
        <obo:IAO_0000115>A reservoir.</obo:IAO_0000115>
        <oboInOwl:hasOBONamespace>GAZ</oboInOwl:hasOBONamespace>
        <oboInOwl:id>GAZ:00239936</oboInOwl:id>
        <rdfs:label>Mankwe Dam Reservoir</rdfs:label>
    </owl:NamedIndividual>
    


    <!-- http://purl.obolibrary.org/obo/GAZ_00239937 -->

    <owl:NamedIndividual rdf:about="http://purl.obolibrary.org/obo/GAZ_00239937">
        <obo:RO_0001025 rdf:resource="http://purl.obolibrary.org/obo/GAZ_00239918"/>
        <obo:IAO_0000115>A reservoir.</obo:IAO_0000115>
        <oboInOwl:hasOBONamespace>GAZ</oboInOwl:hasOBONamespace>
        <oboInOwl:id>GAZ:00239937</oboInOwl:id>
        <rdfs:label>Klipvoor Dam Reservoir</rdfs:label>
    </owl:NamedIndividual>
    


    <!-- http://purl.obolibrary.org/obo/GAZ_00239939 -->

    <owl:NamedIndividual rdf:about="http://purl.obolibrary.org/obo/GAZ_00239939">
        <obo:RO_0001025 rdf:resource="http://purl.obolibrary.org/obo/GAZ_00032877"/>
        <obo:IAO_0000115>A dam. Constructed 1925.</obo:IAO_0000115>
        <oboInOwl:hasOBONamespace>GAZ</oboInOwl:hasOBONamespace>
        <oboInOwl:id>GAZ:00239939</oboInOwl:id>
        <rdfs:label>Hartbeespoort Dam</rdfs:label>
    </owl:NamedIndividual>
    


    <!-- http://purl.obolibrary.org/obo/GAZ_00239942 -->

    <owl:NamedIndividual rdf:about="http://purl.obolibrary.org/obo/GAZ_00239942">
        <obo:IAO_0000115>A dam.</obo:IAO_0000115>
        <oboInOwl:hasOBONamespace>GAZ</oboInOwl:hasOBONamespace>
        <oboInOwl:id>GAZ:00239942</oboInOwl:id>
        <rdfs:label>Van der Kloof Dam</rdfs:label>
    </owl:NamedIndividual>
    


    <!-- http://purl.obolibrary.org/obo/GAZ_00239943 -->

    <owl:NamedIndividual rdf:about="http://purl.obolibrary.org/obo/GAZ_00239943">
        <obo:RO_0001025 rdf:resource="http://purl.obolibrary.org/obo/GAZ_00002818"/>
        <obo:IAO_0000115>A river that drains part of the north eastern Karoo into the Orange River above the Van der Kloof Dam.</obo:IAO_0000115>
        <oboInOwl:hasOBONamespace>GAZ</oboInOwl:hasOBONamespace>
        <oboInOwl:id>GAZ:00239943</oboInOwl:id>
        <rdfs:label>Seekoei River</rdfs:label>
    </owl:NamedIndividual>
    


    <!-- http://purl.obolibrary.org/obo/GAZ_00239944 -->

    <owl:NamedIndividual rdf:about="http://purl.obolibrary.org/obo/GAZ_00239944">
        <obo:RO_0001025 rdf:resource="http://purl.obolibrary.org/obo/GAZ_00002818"/>
        <obo:IAO_0000115>A river. A tributary of the Orange River that rises near Hanover.</obo:IAO_0000115>
        <oboInOwl:hasOBONamespace>GAZ</oboInOwl:hasOBONamespace>
        <oboInOwl:id>GAZ:00239944</oboInOwl:id>
        <rdfs:label>Brak River</rdfs:label>
    </owl:NamedIndividual>
    


    <!-- http://purl.obolibrary.org/obo/GAZ_00239945 -->

    <owl:NamedIndividual rdf:about="http://purl.obolibrary.org/obo/GAZ_00239945">
        <obo:RO_0001025 rdf:resource="http://purl.obolibrary.org/obo/GAZ_00002818"/>
        <obo:IAO_0000115>A river. A tributary of the Brak River that rises near Richmond.</obo:IAO_0000115>
        <oboInOwl:hasOBONamespace>GAZ</oboInOwl:hasOBONamespace>
        <oboInOwl:id>GAZ:00239945</oboInOwl:id>
        <rdfs:label>Ongers River</rdfs:label>
    </owl:NamedIndividual>
    


    <!-- http://purl.obolibrary.org/obo/GAZ_00239946 -->

    <owl:NamedIndividual rdf:about="http://purl.obolibrary.org/obo/GAZ_00239946">
        <obo:RO_0001025 rdf:resource="http://purl.obolibrary.org/obo/GAZ_00002818"/>
        <obo:IAO_0000115>A river. A tributary of the Orange River.</obo:IAO_0000115>
        <oboInOwl:hasOBONamespace>GAZ</oboInOwl:hasOBONamespace>
        <oboInOwl:id>GAZ:00239946</oboInOwl:id>
        <rdfs:label>Hartebeest River</rdfs:label>
    </owl:NamedIndividual>
    


    <!-- http://purl.obolibrary.org/obo/GAZ_00239951 -->

    <owl:NamedIndividual rdf:about="http://purl.obolibrary.org/obo/GAZ_00239951">
        <obo:RO_0001025 rdf:resource="http://purl.obolibrary.org/obo/GAZ_00002818"/>
        <obo:IAO_0000115>A river discharging to the Atlantic Ocean.</obo:IAO_0000115>
        <oboInOwl:hasOBONamespace>GAZ</oboInOwl:hasOBONamespace>
        <oboInOwl:id>GAZ:00239951</oboInOwl:id>
        <rdfs:label>Buffels River</rdfs:label>
    </owl:NamedIndividual>
    


    <!-- http://purl.obolibrary.org/obo/GAZ_00239952 -->

    <owl:NamedIndividual rdf:about="http://purl.obolibrary.org/obo/GAZ_00239952">
        <obo:RO_0001025 rdf:resource="http://purl.obolibrary.org/obo/GAZ_00002818"/>
        <obo:IAO_0000115>A river discharging to the Atlantic Ocean.</obo:IAO_0000115>
        <oboInOwl:hasOBONamespace>GAZ</oboInOwl:hasOBONamespace>
        <oboInOwl:id>GAZ:00239952</oboInOwl:id>
        <rdfs:label>Groen River</rdfs:label>
    </owl:NamedIndividual>
    


    <!-- http://purl.obolibrary.org/obo/GAZ_00239953 -->

    <owl:NamedIndividual rdf:about="http://purl.obolibrary.org/obo/GAZ_00239953">
        <obo:RO_0001025 rdf:resource="http://purl.obolibrary.org/obo/GAZ_00002818"/>
        <obo:IAO_0000115>An archaeological site, formed originally as an ancient solution cavity in Dolomite rocks of the Kuruman Hills, situated between Danielskuil and Kuruman in the Northern Cape Province, South Africa.</obo:IAO_0000115>
        <oboInOwl:hasOBONamespace>GAZ</oboInOwl:hasOBONamespace>
        <oboInOwl:id>GAZ:00239953</oboInOwl:id>
        <rdfs:label>Wonderwerk Cave</rdfs:label>
    </owl:NamedIndividual>
    


    <!-- http://purl.obolibrary.org/obo/GAZ_00239954 -->

    <owl:NamedIndividual rdf:about="http://purl.obolibrary.org/obo/GAZ_00239954">
        <obo:RO_0001025 rdf:resource="http://purl.obolibrary.org/obo/GAZ_00002818"/>
        <obo:IAO_0000115>A protected area located south-west of Kimberley in the Northern Cape, South Africa. Established 2007-06-19.</obo:IAO_0000115>
        <oboInOwl:hasOBONamespace>GAZ</oboInOwl:hasOBONamespace>
        <oboInOwl:id>GAZ:00239954</oboInOwl:id>
        <rdfs:label>Mokala National Park</rdfs:label>
    </owl:NamedIndividual>
    


    <!-- http://purl.obolibrary.org/obo/GAZ_00239955 -->

    <owl:NamedIndividual rdf:about="http://purl.obolibrary.org/obo/GAZ_00239955">
        <obo:RO_0001025 rdf:resource="http://purl.obolibrary.org/obo/GAZ_00002818"/>
        <obo:IAO_0000115>A mountain range in South Africa. Unmarked on many maps of the region, it is in a remote part of the Northern Cape seldom visited by tourists. The range lies between the towns of Calvinia and Sutherland, east and northeast of Tankwa Karoo National Park.</obo:IAO_0000115>
        <oboInOwl:hasOBONamespace>GAZ</oboInOwl:hasOBONamespace>
        <oboInOwl:id>GAZ:00239955</oboInOwl:id>
        <rdfs:label>Roggeveld Mountains</rdfs:label>
    </owl:NamedIndividual>
    


    <!-- http://purl.obolibrary.org/obo/GAZ_00239956 -->

    <owl:NamedIndividual rdf:about="http://purl.obolibrary.org/obo/GAZ_00239956">
        <obo:RO_0001025 rdf:resource="http://purl.obolibrary.org/obo/GAZ_00002817"/>
        <obo:IAO_0000115>A mountain range in South Africa lying south and east of Citrusdal in the Western Cape Province. The range runs north-south, falls within the catchment area of the Olifants River.</obo:IAO_0000115>
        <oboInOwl:hasOBONamespace>GAZ</oboInOwl:hasOBONamespace>
        <oboInOwl:id>GAZ:00239956</oboInOwl:id>
        <rdfs:label>Kouebokkeveld Mountains</rdfs:label>
    </owl:NamedIndividual>
    


    <!-- http://purl.obolibrary.org/obo/GAZ_00239957 -->

    <owl:NamedIndividual rdf:about="http://purl.obolibrary.org/obo/GAZ_00239957">
        <obo:RO_0001025 rdf:resource="http://purl.obolibrary.org/obo/GAZ_00002818"/>
        <obo:IAO_0000115>A protected area.</obo:IAO_0000115>
        <oboInOwl:hasOBONamespace>GAZ</oboInOwl:hasOBONamespace>
        <oboInOwl:id>GAZ:00239957</oboInOwl:id>
        <rdfs:label>Witsand Nature Reserve</rdfs:label>
    </owl:NamedIndividual>
    


    <!-- http://purl.obolibrary.org/obo/GAZ_00239958 -->

    <owl:NamedIndividual rdf:about="http://purl.obolibrary.org/obo/GAZ_00239958">
        <obo:RO_0001025 rdf:resource="http://purl.obolibrary.org/obo/GAZ_00002818"/>
        <obo:IAO_0000115>A protected area.</obo:IAO_0000115>
        <oboInOwl:hasOBONamespace>GAZ</oboInOwl:hasOBONamespace>
        <oboInOwl:id>GAZ:00239958</oboInOwl:id>
        <rdfs:label>Tswalu Kalahari Reserve</rdfs:label>
    </owl:NamedIndividual>
    


    <!-- http://purl.obolibrary.org/obo/GAZ_00239959 -->

    <owl:NamedIndividual rdf:about="http://purl.obolibrary.org/obo/GAZ_00239959">
        <obo:RO_0001025 rdf:resource="http://purl.obolibrary.org/obo/GAZ_00002818"/>
        <obo:IAO_0000115>A protected area.</obo:IAO_0000115>
        <oboInOwl:hasOBONamespace>GAZ</oboInOwl:hasOBONamespace>
        <oboInOwl:id>GAZ:00239959</oboInOwl:id>
        <rdfs:label>Spitskop Nature Reserve</rdfs:label>
    </owl:NamedIndividual>
    


    <!-- http://purl.obolibrary.org/obo/GAZ_00239960 -->

    <owl:NamedIndividual rdf:about="http://purl.obolibrary.org/obo/GAZ_00239960">
        <obo:RO_0001025 rdf:resource="http://purl.obolibrary.org/obo/GAZ_00387367"/>
        <obo:IAO_0000115>A protected area.</obo:IAO_0000115>
        <oboInOwl:hasOBONamespace>GAZ</oboInOwl:hasOBONamespace>
        <oboInOwl:id>GAZ:00239960</oboInOwl:id>
        <rdfs:label>Oorlogskloof Nature Reserve</rdfs:label>
    </owl:NamedIndividual>
    


    <!-- http://purl.obolibrary.org/obo/GAZ_00239961 -->

    <owl:NamedIndividual rdf:about="http://purl.obolibrary.org/obo/GAZ_00239961">
        <obo:RO_0001025 rdf:resource="http://purl.obolibrary.org/obo/GAZ_00032845"/>
        <obo:IAO_0000115>A river in the Western Cape Province of South Africa. Discharges to the Indian Ocean at Witsand.</obo:IAO_0000115>
        <oboInOwl:hasOBONamespace>GAZ</oboInOwl:hasOBONamespace>
        <oboInOwl:id>GAZ:00239961</oboInOwl:id>
        <rdfs:label>Breede River</rdfs:label>
    </owl:NamedIndividual>
    


    <!-- http://purl.obolibrary.org/obo/GAZ_00239970 -->

    <owl:NamedIndividual rdf:about="http://purl.obolibrary.org/obo/GAZ_00239970">
        <obo:IAO_0000115>A dam.</obo:IAO_0000115>
        <oboInOwl:hasOBONamespace>GAZ</oboInOwl:hasOBONamespace>
        <oboInOwl:id>GAZ:00239970</oboInOwl:id>
        <rdfs:label>Clanwilliam Dam</rdfs:label>
    </owl:NamedIndividual>
    


    <!-- http://purl.obolibrary.org/obo/GAZ_00239971 -->

    <owl:NamedIndividual rdf:about="http://purl.obolibrary.org/obo/GAZ_00239971">
        <obo:IAO_0000115>A dam.</obo:IAO_0000115>
        <oboInOwl:hasOBONamespace>GAZ</oboInOwl:hasOBONamespace>
        <oboInOwl:id>GAZ:00239971</oboInOwl:id>
        <rdfs:label>Bulshoek Dam</rdfs:label>
    </owl:NamedIndividual>
    


    <!-- http://purl.obolibrary.org/obo/GAZ_00239972 -->

    <owl:NamedIndividual rdf:about="http://purl.obolibrary.org/obo/GAZ_00239972">
        <obo:RO_0001025 rdf:resource="http://purl.obolibrary.org/obo/GAZ_00076172"/>
        <obo:IAO_0000115>A cave system in the Quaternary limestone formations in the district of Bredasdorp in the Western Cape Province of South Africa.</obo:IAO_0000115>
        <oboInOwl:hasOBONamespace>GAZ</oboInOwl:hasOBONamespace>
        <oboInOwl:id>GAZ:00239972</oboInOwl:id>
        <rdfs:label>Onmeetbarediepgat</rdfs:label>
    </owl:NamedIndividual>
    


    <!-- http://purl.obolibrary.org/obo/GAZ_00239973 -->

    <owl:NamedIndividual rdf:about="http://purl.obolibrary.org/obo/GAZ_00239973">
        <obo:RO_0001025 rdf:resource="http://purl.obolibrary.org/obo/GAZ_00005306"/>
        <obo:IAO_0000115>A part of Cape Town. It is a natural amphitheatre-shaped area bordered by Table Bay and defined by the mountains of Signal Hill, Lion&apos;s Head, Table Mountain and Devil&apos;s Peak.</obo:IAO_0000115>
        <oboInOwl:hasOBONamespace>GAZ</oboInOwl:hasOBONamespace>
        <oboInOwl:id>GAZ:00239973</oboInOwl:id>
        <rdfs:label>City Bowl</rdfs:label>
    </owl:NamedIndividual>
    


    <!-- http://purl.obolibrary.org/obo/GAZ_00239974 -->

    <owl:NamedIndividual rdf:about="http://purl.obolibrary.org/obo/GAZ_00239974">
        <obo:RO_0001025 rdf:resource="http://purl.obolibrary.org/obo/GAZ_00005306"/>
        <obo:IAO_0000115>A part of Cape Town.</obo:IAO_0000115>
        <oboInOwl:hasOBONamespace>GAZ</oboInOwl:hasOBONamespace>
        <oboInOwl:id>GAZ:00239974</oboInOwl:id>
        <rdfs:label>Northern Suburbs</rdfs:label>
    </owl:NamedIndividual>
    


    <!-- http://purl.obolibrary.org/obo/GAZ_00239975 -->

    <owl:NamedIndividual rdf:about="http://purl.obolibrary.org/obo/GAZ_00239975">
        <obo:RO_0001025 rdf:resource="http://purl.obolibrary.org/obo/GAZ_00005306"/>
        <obo:IAO_0000115>A part of Cape Town.</obo:IAO_0000115>
        <oboInOwl:hasOBONamespace>GAZ</oboInOwl:hasOBONamespace>
        <oboInOwl:id>GAZ:00239975</oboInOwl:id>
        <rdfs:label>Atlantic Seaboard</rdfs:label>
    </owl:NamedIndividual>
    


    <!-- http://purl.obolibrary.org/obo/GAZ_00239976 -->

    <owl:NamedIndividual rdf:about="http://purl.obolibrary.org/obo/GAZ_00239976">
        <obo:RO_0001025 rdf:resource="http://purl.obolibrary.org/obo/GAZ_00005306"/>
        <obo:IAO_0000115>A part of Cape Town.</obo:IAO_0000115>
        <oboInOwl:hasOBONamespace>GAZ</oboInOwl:hasOBONamespace>
        <oboInOwl:id>GAZ:00239976</oboInOwl:id>
        <rdfs:label>Southern Suburbs</rdfs:label>
    </owl:NamedIndividual>
    


    <!-- http://purl.obolibrary.org/obo/GAZ_00239977 -->

    <owl:NamedIndividual rdf:about="http://purl.obolibrary.org/obo/GAZ_00239977">
        <obo:RO_0001025 rdf:resource="http://purl.obolibrary.org/obo/GAZ_00005306"/>
        <obo:IAO_0000115>A part of Cape Town.</obo:IAO_0000115>
        <oboInOwl:hasOBONamespace>GAZ</oboInOwl:hasOBONamespace>
        <oboInOwl:id>GAZ:00239977</oboInOwl:id>
        <rdfs:label>South Peninsula</rdfs:label>
    </owl:NamedIndividual>
    


    <!-- http://purl.obolibrary.org/obo/GAZ_00239978 -->

    <owl:NamedIndividual rdf:about="http://purl.obolibrary.org/obo/GAZ_00239978">
        <obo:RO_0001025 rdf:resource="http://purl.obolibrary.org/obo/GAZ_00005306"/>
        <obo:IAO_0000115>A part of Cape Town.</obo:IAO_0000115>
        <oboInOwl:hasOBONamespace>GAZ</oboInOwl:hasOBONamespace>
        <oboInOwl:id>GAZ:00239978</oboInOwl:id>
        <rdfs:label>False Bay</rdfs:label>
    </owl:NamedIndividual>
    


    <!-- http://purl.obolibrary.org/obo/GAZ_00239979 -->

    <owl:NamedIndividual rdf:about="http://purl.obolibrary.org/obo/GAZ_00239979">
        <obo:RO_0001025 rdf:resource="http://purl.obolibrary.org/obo/GAZ_00005306"/>
        <obo:IAO_0000115>A part of Cape Town.</obo:IAO_0000115>
        <oboInOwl:hasOBONamespace>GAZ</oboInOwl:hasOBONamespace>
        <oboInOwl:id>GAZ:00239979</oboInOwl:id>
        <rdfs:label>West Coast</rdfs:label>
    </owl:NamedIndividual>
    


    <!-- http://purl.obolibrary.org/obo/GAZ_00239980 -->

    <owl:NamedIndividual rdf:about="http://purl.obolibrary.org/obo/GAZ_00239980">
        <obo:RO_0001025 rdf:resource="http://purl.obolibrary.org/obo/GAZ_00239976"/>
        <obo:IAO_0000115>A suburb (neighborhood) of Cape Town.</obo:IAO_0000115>
        <oboInOwl:hasOBONamespace>GAZ</oboInOwl:hasOBONamespace>
        <oboInOwl:id>GAZ:00239980</oboInOwl:id>
        <rdfs:label>Bergvliet</rdfs:label>
    </owl:NamedIndividual>
    


    <!-- http://purl.obolibrary.org/obo/GAZ_00239981 -->

    <owl:NamedIndividual rdf:about="http://purl.obolibrary.org/obo/GAZ_00239981">
        <obo:RO_0001025 rdf:resource="http://purl.obolibrary.org/obo/GAZ_00239976"/>
        <obo:IAO_0000115>A suburb (neighborhood) of Cape Town.</obo:IAO_0000115>
        <oboInOwl:hasOBONamespace>GAZ</oboInOwl:hasOBONamespace>
        <oboInOwl:id>GAZ:00239981</oboInOwl:id>
        <rdfs:label>Bishopscourt</rdfs:label>
    </owl:NamedIndividual>
    


    <!-- http://purl.obolibrary.org/obo/GAZ_00239982 -->

    <owl:NamedIndividual rdf:about="http://purl.obolibrary.org/obo/GAZ_00239982">
        <obo:RO_0001025 rdf:resource="http://purl.obolibrary.org/obo/GAZ_00239976"/>
        <obo:IAO_0000115>A suburb (neighborhood) of Cape Town.</obo:IAO_0000115>
        <oboInOwl:hasOBONamespace>GAZ</oboInOwl:hasOBONamespace>
        <oboInOwl:id>GAZ:00239982</oboInOwl:id>
        <rdfs:label>Claremont</rdfs:label>
    </owl:NamedIndividual>
    


    <!-- http://purl.obolibrary.org/obo/GAZ_00239983 -->

    <owl:NamedIndividual rdf:about="http://purl.obolibrary.org/obo/GAZ_00239983">
        <obo:RO_0001025 rdf:resource="http://purl.obolibrary.org/obo/GAZ_00239976"/>
        <obo:IAO_0000115>A suburb (neighborhood) of Cape Town.</obo:IAO_0000115>
        <oboInOwl:hasOBONamespace>GAZ</oboInOwl:hasOBONamespace>
        <oboInOwl:id>GAZ:00239983</oboInOwl:id>
        <rdfs:label>Constantia</rdfs:label>
    </owl:NamedIndividual>
    


    <!-- http://purl.obolibrary.org/obo/GAZ_00239984 -->

    <owl:NamedIndividual rdf:about="http://purl.obolibrary.org/obo/GAZ_00239984">
        <obo:RO_0001025 rdf:resource="http://purl.obolibrary.org/obo/GAZ_00239976"/>
        <obo:IAO_0000115>A suburb (neighborhood) of Cape Town.</obo:IAO_0000115>
        <oboInOwl:hasOBONamespace>GAZ</oboInOwl:hasOBONamespace>
        <oboInOwl:id>GAZ:00239984</oboInOwl:id>
        <rdfs:label>Diep River</rdfs:label>
    </owl:NamedIndividual>
    


    <!-- http://purl.obolibrary.org/obo/GAZ_00239985 -->

    <owl:NamedIndividual rdf:about="http://purl.obolibrary.org/obo/GAZ_00239985">
        <obo:RO_0001025 rdf:resource="http://purl.obolibrary.org/obo/GAZ_00239976"/>
        <obo:IAO_0000115>A suburb (neighborhood) of Cape Town.</obo:IAO_0000115>
        <oboInOwl:hasOBONamespace>GAZ</oboInOwl:hasOBONamespace>
        <oboInOwl:id>GAZ:00239985</oboInOwl:id>
        <rdfs:label>Heathfield</rdfs:label>
    </owl:NamedIndividual>
    


    <!-- http://purl.obolibrary.org/obo/GAZ_00239986 -->

    <owl:NamedIndividual rdf:about="http://purl.obolibrary.org/obo/GAZ_00239986">
        <obo:RO_0001025 rdf:resource="http://purl.obolibrary.org/obo/GAZ_00239976"/>
        <obo:IAO_0000115>A suburb (neighborhood) of Cape Town.</obo:IAO_0000115>
        <oboInOwl:hasOBONamespace>GAZ</oboInOwl:hasOBONamespace>
        <oboInOwl:id>GAZ:00239986</oboInOwl:id>
        <rdfs:label>Kenilworth</rdfs:label>
    </owl:NamedIndividual>
    


    <!-- http://purl.obolibrary.org/obo/GAZ_00239987 -->

    <owl:NamedIndividual rdf:about="http://purl.obolibrary.org/obo/GAZ_00239987">
        <obo:RO_0001025 rdf:resource="http://purl.obolibrary.org/obo/GAZ_00239976"/>
        <obo:IAO_0000115>A suburb (neighborhood) of Cape Town.</obo:IAO_0000115>
        <oboInOwl:hasOBONamespace>GAZ</oboInOwl:hasOBONamespace>
        <oboInOwl:id>GAZ:00239987</oboInOwl:id>
        <rdfs:label>Mowbray</rdfs:label>
    </owl:NamedIndividual>
    


    <!-- http://purl.obolibrary.org/obo/GAZ_00239988 -->

    <owl:NamedIndividual rdf:about="http://purl.obolibrary.org/obo/GAZ_00239988">
        <obo:RO_0001025 rdf:resource="http://purl.obolibrary.org/obo/GAZ_00239976"/>
        <obo:IAO_0000115>A suburb (neighborhood) of Cape Town.</obo:IAO_0000115>
        <oboInOwl:hasOBONamespace>GAZ</oboInOwl:hasOBONamespace>
        <oboInOwl:id>GAZ:00239988</oboInOwl:id>
        <rdfs:label>Newlands</rdfs:label>
    </owl:NamedIndividual>
    


    <!-- http://purl.obolibrary.org/obo/GAZ_00239989 -->

    <owl:NamedIndividual rdf:about="http://purl.obolibrary.org/obo/GAZ_00239989">
        <obo:RO_0001025 rdf:resource="http://purl.obolibrary.org/obo/GAZ_00239976"/>
        <obo:IAO_0000115>A suburb (neighborhood) of Cape Town.</obo:IAO_0000115>
        <oboInOwl:hasOBONamespace>GAZ</oboInOwl:hasOBONamespace>
        <oboInOwl:id>GAZ:00239989</oboInOwl:id>
        <rdfs:label>Observatory</rdfs:label>
    </owl:NamedIndividual>
    


    <!-- http://purl.obolibrary.org/obo/GAZ_00239990 -->

    <owl:NamedIndividual rdf:about="http://purl.obolibrary.org/obo/GAZ_00239990">
        <obo:RO_0001025 rdf:resource="http://purl.obolibrary.org/obo/GAZ_00239976"/>
        <obo:IAO_0000115>A suburb (neighborhood) of Cape Town.</obo:IAO_0000115>
        <oboInOwl:hasOBONamespace>GAZ</oboInOwl:hasOBONamespace>
        <oboInOwl:id>GAZ:00239990</oboInOwl:id>
        <rdfs:label>Pinelands</rdfs:label>
    </owl:NamedIndividual>
    


    <!-- http://purl.obolibrary.org/obo/GAZ_00239991 -->

    <owl:NamedIndividual rdf:about="http://purl.obolibrary.org/obo/GAZ_00239991">
        <obo:RO_0001025 rdf:resource="http://purl.obolibrary.org/obo/GAZ_00239976"/>
        <obo:IAO_0000115>A suburb (neighborhood) of Cape Town.</obo:IAO_0000115>
        <oboInOwl:hasOBONamespace>GAZ</oboInOwl:hasOBONamespace>
        <oboInOwl:id>GAZ:00239991</oboInOwl:id>
        <rdfs:label>Plumstead</rdfs:label>
    </owl:NamedIndividual>
    


    <!-- http://purl.obolibrary.org/obo/GAZ_00239992 -->

    <owl:NamedIndividual rdf:about="http://purl.obolibrary.org/obo/GAZ_00239992">
        <obo:RO_0001025 rdf:resource="http://purl.obolibrary.org/obo/GAZ_00239976"/>
        <obo:IAO_0000115>A suburb (neighborhood) of Cape Town.</obo:IAO_0000115>
        <oboInOwl:hasOBONamespace>GAZ</oboInOwl:hasOBONamespace>
        <oboInOwl:id>GAZ:00239992</oboInOwl:id>
        <rdfs:label>Retreat</rdfs:label>
    </owl:NamedIndividual>
    


    <!-- http://purl.obolibrary.org/obo/GAZ_00239993 -->

    <owl:NamedIndividual rdf:about="http://purl.obolibrary.org/obo/GAZ_00239993">
        <obo:RO_0001025 rdf:resource="http://purl.obolibrary.org/obo/GAZ_00239976"/>
        <obo:IAO_0000115>A suburb (neighborhood) of Cape Town.</obo:IAO_0000115>
        <oboInOwl:hasOBONamespace>GAZ</oboInOwl:hasOBONamespace>
        <oboInOwl:id>GAZ:00239993</oboInOwl:id>
        <rdfs:label>Rondebosch</rdfs:label>
    </owl:NamedIndividual>
    


    <!-- http://purl.obolibrary.org/obo/GAZ_00239994 -->

    <owl:NamedIndividual rdf:about="http://purl.obolibrary.org/obo/GAZ_00239994">
        <obo:RO_0001025 rdf:resource="http://purl.obolibrary.org/obo/GAZ_00239976"/>
        <obo:IAO_0000115>A suburb (neighborhood) of Cape Town.</obo:IAO_0000115>
        <oboInOwl:hasOBONamespace>GAZ</oboInOwl:hasOBONamespace>
        <oboInOwl:id>GAZ:00239994</oboInOwl:id>
        <rdfs:label>Rosebank</rdfs:label>
    </owl:NamedIndividual>
    


    <!-- http://purl.obolibrary.org/obo/GAZ_00239995 -->

    <owl:NamedIndividual rdf:about="http://purl.obolibrary.org/obo/GAZ_00239995">
        <obo:RO_0001025 rdf:resource="http://purl.obolibrary.org/obo/GAZ_00239976"/>
        <obo:IAO_0000115>A suburb (neighborhood) of Cape Town.</obo:IAO_0000115>
        <oboInOwl:hasOBONamespace>GAZ</oboInOwl:hasOBONamespace>
        <oboInOwl:id>GAZ:00239995</oboInOwl:id>
        <rdfs:label>Salt River</rdfs:label>
    </owl:NamedIndividual>
    


    <!-- http://purl.obolibrary.org/obo/GAZ_00239996 -->

    <owl:NamedIndividual rdf:about="http://purl.obolibrary.org/obo/GAZ_00239996">
        <obo:RO_0001025 rdf:resource="http://purl.obolibrary.org/obo/GAZ_00239976"/>
        <obo:IAO_0000115>A suburb (neighborhood) of Cape Town.</obo:IAO_0000115>
        <oboInOwl:hasOBONamespace>GAZ</oboInOwl:hasOBONamespace>
        <oboInOwl:id>GAZ:00239996</oboInOwl:id>
        <rdfs:label>Steenberg</rdfs:label>
    </owl:NamedIndividual>
    


    <!-- http://purl.obolibrary.org/obo/GAZ_00239997 -->

    <owl:NamedIndividual rdf:about="http://purl.obolibrary.org/obo/GAZ_00239997">
        <obo:RO_0001025 rdf:resource="http://purl.obolibrary.org/obo/GAZ_00239976"/>
        <obo:IAO_0000115>A suburb (neighborhood) of Cape Town.</obo:IAO_0000115>
        <oboInOwl:hasOBONamespace>GAZ</oboInOwl:hasOBONamespace>
        <oboInOwl:id>GAZ:00239997</oboInOwl:id>
        <rdfs:label>Tokai</rdfs:label>
    </owl:NamedIndividual>
    


    <!-- http://purl.obolibrary.org/obo/GAZ_00239998 -->

    <owl:NamedIndividual rdf:about="http://purl.obolibrary.org/obo/GAZ_00239998">
        <obo:RO_0001025 rdf:resource="http://purl.obolibrary.org/obo/GAZ_00239976"/>
        <obo:IAO_0000115>A suburb (neighborhood) of Cape Town.</obo:IAO_0000115>
        <oboInOwl:hasOBONamespace>GAZ</oboInOwl:hasOBONamespace>
        <oboInOwl:id>GAZ:00239998</oboInOwl:id>
        <rdfs:label>Woodstock</rdfs:label>
    </owl:NamedIndividual>
    


    <!-- http://purl.obolibrary.org/obo/GAZ_00239999 -->

    <owl:NamedIndividual rdf:about="http://purl.obolibrary.org/obo/GAZ_00239999">
        <obo:RO_0001025 rdf:resource="http://purl.obolibrary.org/obo/GAZ_00239976"/>
        <obo:IAO_0000115>A suburb (neighborhood) of Cape Town.</obo:IAO_0000115>
        <oboInOwl:hasOBONamespace>GAZ</oboInOwl:hasOBONamespace>
        <oboInOwl:id>GAZ:00239999</oboInOwl:id>
        <rdfs:label>Wynberg</rdfs:label>
    </owl:NamedIndividual>
    


    <!-- http://purl.obolibrary.org/obo/GAZ_00240000 -->

    <owl:NamedIndividual rdf:about="http://purl.obolibrary.org/obo/GAZ_00240000">
        <obo:RO_0001025 rdf:resource="http://purl.obolibrary.org/obo/GAZ_00239979"/>
        <obo:IAO_0000115>A suburb (neighborhood) of Cape Town.</obo:IAO_0000115>
        <oboInOwl:hasOBONamespace>GAZ</oboInOwl:hasOBONamespace>
        <oboInOwl:id>GAZ:00240000</oboInOwl:id>
        <rdfs:label>Bloubergstrand</rdfs:label>
    </owl:NamedIndividual>
    


    <!-- http://purl.obolibrary.org/obo/GAZ_00240001 -->

    <owl:NamedIndividual rdf:about="http://purl.obolibrary.org/obo/GAZ_00240001">
        <obo:RO_0001025 rdf:resource="http://purl.obolibrary.org/obo/GAZ_00239979"/>
        <obo:IAO_0000115>A suburb (neighborhood) of Cape Town.</obo:IAO_0000115>
        <oboInOwl:hasOBONamespace>GAZ</oboInOwl:hasOBONamespace>
        <oboInOwl:id>GAZ:00240001</oboInOwl:id>
        <rdfs:label>Milnerton</rdfs:label>
    </owl:NamedIndividual>
    


    <!-- http://purl.obolibrary.org/obo/GAZ_00240002 -->

    <owl:NamedIndividual rdf:about="http://purl.obolibrary.org/obo/GAZ_00240002">
        <obo:RO_0001025 rdf:resource="http://purl.obolibrary.org/obo/GAZ_00239979"/>
        <obo:IAO_0000115>A suburb (neighborhood) of Cape Town.</obo:IAO_0000115>
        <oboInOwl:hasOBONamespace>GAZ</oboInOwl:hasOBONamespace>
        <oboInOwl:id>GAZ:00240002</oboInOwl:id>
        <rdfs:label>Parklands</rdfs:label>
    </owl:NamedIndividual>
    


    <!-- http://purl.obolibrary.org/obo/GAZ_00240003 -->

    <owl:NamedIndividual rdf:about="http://purl.obolibrary.org/obo/GAZ_00240003">
        <obo:RO_0001025 rdf:resource="http://purl.obolibrary.org/obo/GAZ_00239979"/>
        <obo:IAO_0000115>A suburb (neighborhood) of Cape Town.</obo:IAO_0000115>
        <oboInOwl:hasOBONamespace>GAZ</oboInOwl:hasOBONamespace>
        <oboInOwl:id>GAZ:00240003</oboInOwl:id>
        <rdfs:label>Tableview</rdfs:label>
    </owl:NamedIndividual>
    


    <!-- http://purl.obolibrary.org/obo/GAZ_00240004 -->

    <owl:NamedIndividual rdf:about="http://purl.obolibrary.org/obo/GAZ_00240004">
        <obo:RO_0001025 rdf:resource="http://purl.obolibrary.org/obo/GAZ_00239979"/>
        <obo:IAO_0000115>A suburb (neighborhood) of Cape Town.</obo:IAO_0000115>
        <oboInOwl:hasOBONamespace>GAZ</oboInOwl:hasOBONamespace>
        <oboInOwl:id>GAZ:00240004</oboInOwl:id>
        <rdfs:label>Melkbosstrand</rdfs:label>
    </owl:NamedIndividual>
    


    <!-- http://purl.obolibrary.org/obo/GAZ_00240006 -->

    <owl:NamedIndividual rdf:about="http://purl.obolibrary.org/obo/GAZ_00240006">
        <obo:RO_0001025 rdf:resource="http://purl.obolibrary.org/obo/GAZ_00240001"/>
        <obo:IAO_0000115>A lagoon at the estuary of the Diep River.</obo:IAO_0000115>
        <oboInOwl:hasOBONamespace>GAZ</oboInOwl:hasOBONamespace>
        <oboInOwl:id>GAZ:00240006</oboInOwl:id>
        <rdfs:label>Milnerton Lagoon</rdfs:label>
    </owl:NamedIndividual>
    


    <!-- http://purl.obolibrary.org/obo/GAZ_00240007 -->

    <owl:NamedIndividual rdf:about="http://purl.obolibrary.org/obo/GAZ_00240007">
        <obo:RO_0001025 rdf:resource="http://purl.obolibrary.org/obo/GAZ_00009437"/>
        <obo:IAO_0000115>A river discharging to Table Bay.</obo:IAO_0000115>
        <oboInOwl:hasOBONamespace>GAZ</oboInOwl:hasOBONamespace>
        <oboInOwl:id>GAZ:00240007</oboInOwl:id>
        <rdfs:label>Black River</rdfs:label>
    </owl:NamedIndividual>
    


    <!-- http://purl.obolibrary.org/obo/GAZ_00240009 -->

    <owl:NamedIndividual rdf:about="http://purl.obolibrary.org/obo/GAZ_00240009">
        <obo:RO_0001025 rdf:resource="http://purl.obolibrary.org/obo/GAZ_00076275"/>
        <obo:RO_0001025 rdf:resource="http://purl.obolibrary.org/obo/GAZ_00239988"/>
        <obo:IAO_0000115>A forest.</obo:IAO_0000115>
        <oboInOwl:hasOBONamespace>GAZ</oboInOwl:hasOBONamespace>
        <oboInOwl:id>GAZ:00240009</oboInOwl:id>
        <rdfs:label>Newlands Forest</rdfs:label>
    </owl:NamedIndividual>
    


    <!-- http://purl.obolibrary.org/obo/GAZ_00240010 -->

    <owl:NamedIndividual rdf:about="http://purl.obolibrary.org/obo/GAZ_00240010">
        <obo:RO_0001025 rdf:resource="http://purl.obolibrary.org/obo/GAZ_00239978"/>
        <obo:IAO_0000115>A suburb (neighborhood) of Cape Town.</obo:IAO_0000115>
        <oboInOwl:hasOBONamespace>GAZ</oboInOwl:hasOBONamespace>
        <oboInOwl:id>GAZ:00240010</oboInOwl:id>
        <rdfs:label>Gordon&apos;s Bay</rdfs:label>
    </owl:NamedIndividual>
    


    <!-- http://purl.obolibrary.org/obo/GAZ_00240011 -->

    <owl:NamedIndividual rdf:about="http://purl.obolibrary.org/obo/GAZ_00240011">
        <obo:RO_0001025 rdf:resource="http://purl.obolibrary.org/obo/GAZ_00239978"/>
        <obo:IAO_0000115>A suburb (neighborhood) of Cape Town.</obo:IAO_0000115>
        <oboInOwl:hasOBONamespace>GAZ</oboInOwl:hasOBONamespace>
        <oboInOwl:id>GAZ:00240011</oboInOwl:id>
        <rdfs:label>Somerset West</rdfs:label>
    </owl:NamedIndividual>
    


    <!-- http://purl.obolibrary.org/obo/GAZ_00240012 -->

    <owl:NamedIndividual rdf:about="http://purl.obolibrary.org/obo/GAZ_00240012">
        <obo:RO_0001025 rdf:resource="http://purl.obolibrary.org/obo/GAZ_00239978"/>
        <obo:IAO_0000115>A suburb (neighborhood) of Cape Town.</obo:IAO_0000115>
        <oboInOwl:hasOBONamespace>GAZ</oboInOwl:hasOBONamespace>
        <oboInOwl:id>GAZ:00240012</oboInOwl:id>
        <rdfs:label>Strand</rdfs:label>
    </owl:NamedIndividual>
    


    <!-- http://purl.obolibrary.org/obo/GAZ_00240013 -->

    <owl:NamedIndividual rdf:about="http://purl.obolibrary.org/obo/GAZ_00240013">
        <obo:RO_0001025 rdf:resource="http://purl.obolibrary.org/obo/GAZ_00076136"/>
        <obo:IAO_0000115>A dam in the Hottentots-Holland mountains near Cape Town in South Africa. Completed 1979.</obo:IAO_0000115>
        <oboInOwl:hasOBONamespace>GAZ</oboInOwl:hasOBONamespace>
        <oboInOwl:id>GAZ:00240013</oboInOwl:id>
        <rdfs:label>Steenbras Dam</rdfs:label>
    </owl:NamedIndividual>
    


    <!-- http://purl.obolibrary.org/obo/GAZ_00240014 -->

    <owl:NamedIndividual rdf:about="http://purl.obolibrary.org/obo/GAZ_00240014">
        <obo:RO_0001025 rdf:resource="http://purl.obolibrary.org/obo/GAZ_00240011"/>
        <obo:IAO_0000115>A protected area.</obo:IAO_0000115>
        <oboInOwl:hasOBONamespace>GAZ</oboInOwl:hasOBONamespace>
        <oboInOwl:id>GAZ:00240014</oboInOwl:id>
        <rdfs:label>Helderberg Nature Reserve</rdfs:label>
    </owl:NamedIndividual>
    


    <!-- http://purl.obolibrary.org/obo/GAZ_00240015 -->

    <owl:NamedIndividual rdf:about="http://purl.obolibrary.org/obo/GAZ_00240015">
        <obo:RO_0001025 rdf:resource="http://purl.obolibrary.org/obo/GAZ_00058871"/>
        <obo:IAO_0000115>A suburb (neighborhood) of Cape Town.</obo:IAO_0000115>
        <oboInOwl:hasOBONamespace>GAZ</oboInOwl:hasOBONamespace>
        <oboInOwl:id>GAZ:00240015</oboInOwl:id>
        <rdfs:label>Athlone</rdfs:label>
    </owl:NamedIndividual>
    


    <!-- http://purl.obolibrary.org/obo/GAZ_00240016 -->

    <owl:NamedIndividual rdf:about="http://purl.obolibrary.org/obo/GAZ_00240016">
        <obo:RO_0001025 rdf:resource="http://purl.obolibrary.org/obo/GAZ_00058871"/>
        <obo:IAO_0000115>A suburb (neighborhood) of Cape Town.</obo:IAO_0000115>
        <oboInOwl:hasOBONamespace>GAZ</oboInOwl:hasOBONamespace>
        <oboInOwl:id>GAZ:00240016</oboInOwl:id>
        <rdfs:label>Belhar</rdfs:label>
    </owl:NamedIndividual>
    


    <!-- http://purl.obolibrary.org/obo/GAZ_00240017 -->

    <owl:NamedIndividual rdf:about="http://purl.obolibrary.org/obo/GAZ_00240017">
        <obo:RO_0001025 rdf:resource="http://purl.obolibrary.org/obo/GAZ_00058871"/>
        <obo:IAO_0000115>A suburb (neighborhood) of Cape Town.</obo:IAO_0000115>
        <oboInOwl:hasOBONamespace>GAZ</oboInOwl:hasOBONamespace>
        <oboInOwl:id>GAZ:00240017</oboInOwl:id>
        <rdfs:label>Blue Downs</rdfs:label>
    </owl:NamedIndividual>
    


    <!-- http://purl.obolibrary.org/obo/GAZ_00240018 -->

    <owl:NamedIndividual rdf:about="http://purl.obolibrary.org/obo/GAZ_00240018">
        <obo:RO_0001025 rdf:resource="http://purl.obolibrary.org/obo/GAZ_00058871"/>
        <obo:IAO_0000115>A suburb (neighborhood) of Cape Town.</obo:IAO_0000115>
        <oboInOwl:hasOBONamespace>GAZ</oboInOwl:hasOBONamespace>
        <oboInOwl:id>GAZ:00240018</oboInOwl:id>
        <rdfs:label>Bonteheuwel</rdfs:label>
    </owl:NamedIndividual>
    


    <!-- http://purl.obolibrary.org/obo/GAZ_00240019 -->

    <owl:NamedIndividual rdf:about="http://purl.obolibrary.org/obo/GAZ_00240019">
        <obo:RO_0001025 rdf:resource="http://purl.obolibrary.org/obo/GAZ_00058871"/>
        <obo:IAO_0000115>A suburb (neighborhood) of Cape Town.</obo:IAO_0000115>
        <oboInOwl:hasOBONamespace>GAZ</oboInOwl:hasOBONamespace>
        <oboInOwl:id>GAZ:00240019</oboInOwl:id>
        <rdfs:label>Crawford</rdfs:label>
    </owl:NamedIndividual>
    


    <!-- http://purl.obolibrary.org/obo/GAZ_00240020 -->

    <owl:NamedIndividual rdf:about="http://purl.obolibrary.org/obo/GAZ_00240020">
        <obo:RO_0001025 rdf:resource="http://purl.obolibrary.org/obo/GAZ_00058871"/>
        <obo:IAO_0000115>A suburb (neighborhood) of Cape Town.</obo:IAO_0000115>
        <oboInOwl:hasOBONamespace>GAZ</oboInOwl:hasOBONamespace>
        <oboInOwl:id>GAZ:00240020</oboInOwl:id>
        <rdfs:label>Crossroads</rdfs:label>
    </owl:NamedIndividual>
    


    <!-- http://purl.obolibrary.org/obo/GAZ_00240021 -->

    <owl:NamedIndividual rdf:about="http://purl.obolibrary.org/obo/GAZ_00240021">
        <obo:RO_0001025 rdf:resource="http://purl.obolibrary.org/obo/GAZ_00058871"/>
        <obo:IAO_0000115>A suburb (neighborhood) of Cape Town.</obo:IAO_0000115>
        <oboInOwl:hasOBONamespace>GAZ</oboInOwl:hasOBONamespace>
        <oboInOwl:id>GAZ:00240021</oboInOwl:id>
        <rdfs:label>Delft</rdfs:label>
    </owl:NamedIndividual>
    


    <!-- http://purl.obolibrary.org/obo/GAZ_00240022 -->

    <owl:NamedIndividual rdf:about="http://purl.obolibrary.org/obo/GAZ_00240022">
        <obo:RO_0001025 rdf:resource="http://purl.obolibrary.org/obo/GAZ_00058871"/>
        <obo:IAO_0000115>A suburb (neighborhood) of Cape Town.</obo:IAO_0000115>
        <oboInOwl:hasOBONamespace>GAZ</oboInOwl:hasOBONamespace>
        <oboInOwl:id>GAZ:00240022</oboInOwl:id>
        <rdfs:label>Elsie&apos;s River</rdfs:label>
    </owl:NamedIndividual>
    


    <!-- http://purl.obolibrary.org/obo/GAZ_00240023 -->

    <owl:NamedIndividual rdf:about="http://purl.obolibrary.org/obo/GAZ_00240023">
        <obo:RO_0001025 rdf:resource="http://purl.obolibrary.org/obo/GAZ_00058871"/>
        <obo:IAO_0000115>A suburb (neighborhood) of Cape Town.</obo:IAO_0000115>
        <oboInOwl:hasOBONamespace>GAZ</oboInOwl:hasOBONamespace>
        <oboInOwl:id>GAZ:00240023</oboInOwl:id>
        <rdfs:label>Epping</rdfs:label>
    </owl:NamedIndividual>
    


    <!-- http://purl.obolibrary.org/obo/GAZ_00240024 -->

    <owl:NamedIndividual rdf:about="http://purl.obolibrary.org/obo/GAZ_00240024">
        <obo:RO_0001025 rdf:resource="http://purl.obolibrary.org/obo/GAZ_00058871"/>
        <obo:IAO_0000115>A suburb (neighborhood) of Cape Town.</obo:IAO_0000115>
        <oboInOwl:hasOBONamespace>GAZ</oboInOwl:hasOBONamespace>
        <oboInOwl:id>GAZ:00240024</oboInOwl:id>
        <rdfs:label>Grassy Park</rdfs:label>
    </owl:NamedIndividual>
    


    <!-- http://purl.obolibrary.org/obo/GAZ_00240025 -->

    <owl:NamedIndividual rdf:about="http://purl.obolibrary.org/obo/GAZ_00240025">
        <obo:RO_0001025 rdf:resource="http://purl.obolibrary.org/obo/GAZ_00058871"/>
        <obo:IAO_0000115>A suburb (neighborhood) of Cape Town.</obo:IAO_0000115>
        <oboInOwl:hasOBONamespace>GAZ</oboInOwl:hasOBONamespace>
        <oboInOwl:id>GAZ:00240025</oboInOwl:id>
        <rdfs:label>Gugulethu</rdfs:label>
    </owl:NamedIndividual>
    


    <!-- http://purl.obolibrary.org/obo/GAZ_00240026 -->

    <owl:NamedIndividual rdf:about="http://purl.obolibrary.org/obo/GAZ_00240026">
        <obo:RO_0001025 rdf:resource="http://purl.obolibrary.org/obo/GAZ_00058871"/>
        <obo:IAO_0000115>A suburb (neighborhood) of Cape Town.</obo:IAO_0000115>
        <oboInOwl:hasOBONamespace>GAZ</oboInOwl:hasOBONamespace>
        <oboInOwl:id>GAZ:00240026</oboInOwl:id>
        <rdfs:label>Khayelitsha</rdfs:label>
    </owl:NamedIndividual>
    


    <!-- http://purl.obolibrary.org/obo/GAZ_00240027 -->

    <owl:NamedIndividual rdf:about="http://purl.obolibrary.org/obo/GAZ_00240027">
        <obo:RO_0001025 rdf:resource="http://purl.obolibrary.org/obo/GAZ_00058871"/>
        <obo:IAO_0000115>A suburb (neighborhood) of Cape Town.</obo:IAO_0000115>
        <oboInOwl:hasOBONamespace>GAZ</oboInOwl:hasOBONamespace>
        <oboInOwl:id>GAZ:00240027</oboInOwl:id>
        <rdfs:label>Langa</rdfs:label>
    </owl:NamedIndividual>
    


    <!-- http://purl.obolibrary.org/obo/GAZ_00240028 -->

    <owl:NamedIndividual rdf:about="http://purl.obolibrary.org/obo/GAZ_00240028">
        <obo:RO_0001025 rdf:resource="http://purl.obolibrary.org/obo/GAZ_00058871"/>
        <obo:IAO_0000115>A suburb (neighborhood) of Cape Town.</obo:IAO_0000115>
        <oboInOwl:hasOBONamespace>GAZ</oboInOwl:hasOBONamespace>
        <oboInOwl:id>GAZ:00240028</oboInOwl:id>
        <rdfs:label>Lansdowne</rdfs:label>
    </owl:NamedIndividual>
    


    <!-- http://purl.obolibrary.org/obo/GAZ_00240029 -->

    <owl:NamedIndividual rdf:about="http://purl.obolibrary.org/obo/GAZ_00240029">
        <obo:RO_0001025 rdf:resource="http://purl.obolibrary.org/obo/GAZ_00058871"/>
        <obo:IAO_0000115>A suburb (neighborhood) of Cape Town.</obo:IAO_0000115>
        <oboInOwl:hasOBONamespace>GAZ</oboInOwl:hasOBONamespace>
        <oboInOwl:id>GAZ:00240029</oboInOwl:id>
        <rdfs:label>Lotus River</rdfs:label>
    </owl:NamedIndividual>
    


    <!-- http://purl.obolibrary.org/obo/GAZ_00240030 -->

    <owl:NamedIndividual rdf:about="http://purl.obolibrary.org/obo/GAZ_00240030">
        <obo:RO_0001025 rdf:resource="http://purl.obolibrary.org/obo/GAZ_00058871"/>
        <obo:IAO_0000115>A suburb (neighborhood) of Cape Town.</obo:IAO_0000115>
        <oboInOwl:hasOBONamespace>GAZ</oboInOwl:hasOBONamespace>
        <oboInOwl:id>GAZ:00240030</oboInOwl:id>
        <rdfs:label>Manenberg</rdfs:label>
    </owl:NamedIndividual>
    


    <!-- http://purl.obolibrary.org/obo/GAZ_00240031 -->

    <owl:NamedIndividual rdf:about="http://purl.obolibrary.org/obo/GAZ_00240031">
        <obo:RO_0001025 rdf:resource="http://purl.obolibrary.org/obo/GAZ_00058871"/>
        <obo:IAO_0000115>A suburb (neighborhood) of Cape Town.</obo:IAO_0000115>
        <oboInOwl:hasOBONamespace>GAZ</oboInOwl:hasOBONamespace>
        <oboInOwl:id>GAZ:00240031</oboInOwl:id>
        <rdfs:label>Mfuleni</rdfs:label>
    </owl:NamedIndividual>
    


    <!-- http://purl.obolibrary.org/obo/GAZ_00240032 -->

    <owl:NamedIndividual rdf:about="http://purl.obolibrary.org/obo/GAZ_00240032">
        <obo:RO_0001025 rdf:resource="http://purl.obolibrary.org/obo/GAZ_00058871"/>
        <obo:IAO_0000115>A suburb (neighborhood) of Cape Town.</obo:IAO_0000115>
        <oboInOwl:hasOBONamespace>GAZ</oboInOwl:hasOBONamespace>
        <oboInOwl:id>GAZ:00240032</oboInOwl:id>
        <rdfs:label>Mitchell&apos;s Plain</rdfs:label>
    </owl:NamedIndividual>
    


    <!-- http://purl.obolibrary.org/obo/GAZ_00240033 -->

    <owl:NamedIndividual rdf:about="http://purl.obolibrary.org/obo/GAZ_00240033">
        <obo:RO_0001025 rdf:resource="http://purl.obolibrary.org/obo/GAZ_00058871"/>
        <obo:IAO_0000115>A suburb (neighborhood) of Cape Town.</obo:IAO_0000115>
        <oboInOwl:hasOBONamespace>GAZ</oboInOwl:hasOBONamespace>
        <oboInOwl:id>GAZ:00240033</oboInOwl:id>
        <rdfs:label>Nyanga</rdfs:label>
    </owl:NamedIndividual>
    


    <!-- http://purl.obolibrary.org/obo/GAZ_00240034 -->

    <owl:NamedIndividual rdf:about="http://purl.obolibrary.org/obo/GAZ_00240034">
        <obo:RO_0001025 rdf:resource="http://purl.obolibrary.org/obo/GAZ_00058871"/>
        <obo:IAO_0000115>A suburb (neighborhood) of Cape Town.</obo:IAO_0000115>
        <oboInOwl:hasOBONamespace>GAZ</oboInOwl:hasOBONamespace>
        <oboInOwl:id>GAZ:00240034</oboInOwl:id>
        <rdfs:label>Ottery</rdfs:label>
    </owl:NamedIndividual>
    


    <!-- http://purl.obolibrary.org/obo/GAZ_00240035 -->

    <owl:NamedIndividual rdf:about="http://purl.obolibrary.org/obo/GAZ_00240035">
        <obo:RO_0001025 rdf:resource="http://purl.obolibrary.org/obo/GAZ_00058871"/>
        <obo:IAO_0000115>A suburb (neighborhood) of Cape Town.</obo:IAO_0000115>
        <oboInOwl:hasOBONamespace>GAZ</oboInOwl:hasOBONamespace>
        <oboInOwl:id>GAZ:00240035</oboInOwl:id>
        <rdfs:label>Philippi</rdfs:label>
    </owl:NamedIndividual>
    


    <!-- http://purl.obolibrary.org/obo/GAZ_00240036 -->

    <owl:NamedIndividual rdf:about="http://purl.obolibrary.org/obo/GAZ_00240036">
        <obo:RO_0001025 rdf:resource="http://purl.obolibrary.org/obo/GAZ_00058871"/>
        <obo:IAO_0000115>A suburb (neighborhood) of Cape Town.</obo:IAO_0000115>
        <oboInOwl:hasOBONamespace>GAZ</oboInOwl:hasOBONamespace>
        <oboInOwl:id>GAZ:00240036</oboInOwl:id>
        <rdfs:label>Wetton</rdfs:label>
    </owl:NamedIndividual>
    


    <!-- http://purl.obolibrary.org/obo/GAZ_00240037 -->

    <owl:NamedIndividual rdf:about="http://purl.obolibrary.org/obo/GAZ_00240037">
        <obo:RO_0001025 rdf:resource="http://purl.obolibrary.org/obo/GAZ_00239977"/>
        <obo:IAO_0000115>A suburb (neighborhood) of Cape Town.</obo:IAO_0000115>
        <oboInOwl:hasOBONamespace>GAZ</oboInOwl:hasOBONamespace>
        <oboInOwl:id>GAZ:00240037</oboInOwl:id>
        <rdfs:label>Capri Village</rdfs:label>
    </owl:NamedIndividual>
    


    <!-- http://purl.obolibrary.org/obo/GAZ_00240038 -->

    <owl:NamedIndividual rdf:about="http://purl.obolibrary.org/obo/GAZ_00240038">
        <obo:RO_0001025 rdf:resource="http://purl.obolibrary.org/obo/GAZ_00239977"/>
        <obo:IAO_0000115>A suburb (neighborhood) of Cape Town.</obo:IAO_0000115>
        <oboInOwl:hasOBONamespace>GAZ</oboInOwl:hasOBONamespace>
        <oboInOwl:id>GAZ:00240038</oboInOwl:id>
        <rdfs:label>Clovelly</rdfs:label>
    </owl:NamedIndividual>
    


    <!-- http://purl.obolibrary.org/obo/GAZ_00240039 -->

    <owl:NamedIndividual rdf:about="http://purl.obolibrary.org/obo/GAZ_00240039">
        <obo:RO_0001025 rdf:resource="http://purl.obolibrary.org/obo/GAZ_00239977"/>
        <obo:IAO_0000115>A suburb (neighborhood) of Cape Town.</obo:IAO_0000115>
        <oboInOwl:hasOBONamespace>GAZ</oboInOwl:hasOBONamespace>
        <oboInOwl:id>GAZ:00240039</oboInOwl:id>
        <rdfs:label>Fish Hoek</rdfs:label>
    </owl:NamedIndividual>
    


    <!-- http://purl.obolibrary.org/obo/GAZ_00240040 -->

    <owl:NamedIndividual rdf:about="http://purl.obolibrary.org/obo/GAZ_00240040">
        <obo:RO_0001025 rdf:resource="http://purl.obolibrary.org/obo/GAZ_00239977"/>
        <obo:IAO_0000115>A suburb (neighborhood) of Cape Town.</obo:IAO_0000115>
        <oboInOwl:hasOBONamespace>GAZ</oboInOwl:hasOBONamespace>
        <oboInOwl:id>GAZ:00240040</oboInOwl:id>
        <rdfs:label>Glencairn</rdfs:label>
    </owl:NamedIndividual>
    


    <!-- http://purl.obolibrary.org/obo/GAZ_00240041 -->

    <owl:NamedIndividual rdf:about="http://purl.obolibrary.org/obo/GAZ_00240041">
        <obo:RO_0001025 rdf:resource="http://purl.obolibrary.org/obo/GAZ_00239977"/>
        <obo:IAO_0000115>A suburb (neighborhood) of Cape Town.</obo:IAO_0000115>
        <oboInOwl:hasOBONamespace>GAZ</oboInOwl:hasOBONamespace>
        <oboInOwl:id>GAZ:00240041</oboInOwl:id>
        <rdfs:label>Kalk Bay</rdfs:label>
    </owl:NamedIndividual>
    


    <!-- http://purl.obolibrary.org/obo/GAZ_00240042 -->

    <owl:NamedIndividual rdf:about="http://purl.obolibrary.org/obo/GAZ_00240042">
        <obo:RO_0001025 rdf:resource="http://purl.obolibrary.org/obo/GAZ_00239977"/>
        <obo:IAO_0000115>A suburb (neighborhood) of Cape Town.</obo:IAO_0000115>
        <oboInOwl:hasOBONamespace>GAZ</oboInOwl:hasOBONamespace>
        <oboInOwl:id>GAZ:00240042</oboInOwl:id>
        <rdfs:label>Kommetjie</rdfs:label>
    </owl:NamedIndividual>
    


    <!-- http://purl.obolibrary.org/obo/GAZ_00240043 -->

    <owl:NamedIndividual rdf:about="http://purl.obolibrary.org/obo/GAZ_00240043">
        <obo:RO_0001025 rdf:resource="http://purl.obolibrary.org/obo/GAZ_00239977"/>
        <obo:IAO_0000115>A suburb (neighborhood) of Cape Town.</obo:IAO_0000115>
        <oboInOwl:hasOBONamespace>GAZ</oboInOwl:hasOBONamespace>
        <oboInOwl:id>GAZ:00240043</oboInOwl:id>
        <rdfs:label>Masiphumelele</rdfs:label>
    </owl:NamedIndividual>
    


    <!-- http://purl.obolibrary.org/obo/GAZ_00240044 -->

    <owl:NamedIndividual rdf:about="http://purl.obolibrary.org/obo/GAZ_00240044">
        <obo:RO_0001025 rdf:resource="http://purl.obolibrary.org/obo/GAZ_00239977"/>
        <obo:IAO_0000115>A suburb (neighborhood) of Cape Town.</obo:IAO_0000115>
        <oboInOwl:hasOBONamespace>GAZ</oboInOwl:hasOBONamespace>
        <oboInOwl:id>GAZ:00240044</oboInOwl:id>
        <rdfs:label>Muizenberg</rdfs:label>
    </owl:NamedIndividual>
    


    <!-- http://purl.obolibrary.org/obo/GAZ_00240045 -->

    <owl:NamedIndividual rdf:about="http://purl.obolibrary.org/obo/GAZ_00240045">
        <obo:RO_0001025 rdf:resource="http://purl.obolibrary.org/obo/GAZ_00239977"/>
        <obo:IAO_0000115>A suburb (neighborhood) of Cape Town.</obo:IAO_0000115>
        <oboInOwl:hasOBONamespace>GAZ</oboInOwl:hasOBONamespace>
        <oboInOwl:id>GAZ:00240045</oboInOwl:id>
        <rdfs:label>Noordhoek</rdfs:label>
    </owl:NamedIndividual>
    


    <!-- http://purl.obolibrary.org/obo/GAZ_00240046 -->

    <owl:NamedIndividual rdf:about="http://purl.obolibrary.org/obo/GAZ_00240046">
        <obo:RO_0001025 rdf:resource="http://purl.obolibrary.org/obo/GAZ_00239977"/>
        <obo:IAO_0000115>A suburb (neighborhood) of Cape Town.</obo:IAO_0000115>
        <oboInOwl:hasOBONamespace>GAZ</oboInOwl:hasOBONamespace>
        <oboInOwl:id>GAZ:00240046</oboInOwl:id>
        <rdfs:label>Ocean View</rdfs:label>
    </owl:NamedIndividual>
    


    <!-- http://purl.obolibrary.org/obo/GAZ_00240047 -->

    <owl:NamedIndividual rdf:about="http://purl.obolibrary.org/obo/GAZ_00240047">
        <obo:RO_0001025 rdf:resource="http://purl.obolibrary.org/obo/GAZ_00239977"/>
        <obo:IAO_0000115>A suburb (neighborhood) of Cape Town.</obo:IAO_0000115>
        <oboInOwl:hasOBONamespace>GAZ</oboInOwl:hasOBONamespace>
        <oboInOwl:id>GAZ:00240047</oboInOwl:id>
        <rdfs:label>Scarborough</rdfs:label>
    </owl:NamedIndividual>
    


    <!-- http://purl.obolibrary.org/obo/GAZ_00240048 -->

    <owl:NamedIndividual rdf:about="http://purl.obolibrary.org/obo/GAZ_00240048">
        <obo:RO_0001025 rdf:resource="http://purl.obolibrary.org/obo/GAZ_00239977"/>
        <obo:IAO_0000115>A suburb (neighborhood) of Cape Town.</obo:IAO_0000115>
        <oboInOwl:hasOBONamespace>GAZ</oboInOwl:hasOBONamespace>
        <oboInOwl:id>GAZ:00240048</oboInOwl:id>
        <rdfs:label>Simon&apos;s Town</rdfs:label>
    </owl:NamedIndividual>
    


    <!-- http://purl.obolibrary.org/obo/GAZ_00240049 -->

    <owl:NamedIndividual rdf:about="http://purl.obolibrary.org/obo/GAZ_00240049">
        <obo:RO_0001025 rdf:resource="http://purl.obolibrary.org/obo/GAZ_00239977"/>
        <obo:IAO_0000115>A suburb (neighborhood) of Cape Town.</obo:IAO_0000115>
        <oboInOwl:hasOBONamespace>GAZ</oboInOwl:hasOBONamespace>
        <oboInOwl:id>GAZ:00240049</oboInOwl:id>
        <rdfs:label>Saint James</rdfs:label>
    </owl:NamedIndividual>
    


    <!-- http://purl.obolibrary.org/obo/GAZ_00240050 -->

    <owl:NamedIndividual rdf:about="http://purl.obolibrary.org/obo/GAZ_00240050">
        <obo:RO_0001025 rdf:resource="http://purl.obolibrary.org/obo/GAZ_00239977"/>
        <obo:IAO_0000115>A suburb (neighborhood) of Cape Town.</obo:IAO_0000115>
        <oboInOwl:hasOBONamespace>GAZ</oboInOwl:hasOBONamespace>
        <oboInOwl:id>GAZ:00240050</oboInOwl:id>
        <rdfs:label>Sunnydale</rdfs:label>
    </owl:NamedIndividual>
    


    <!-- http://purl.obolibrary.org/obo/GAZ_00240051 -->

    <owl:NamedIndividual rdf:about="http://purl.obolibrary.org/obo/GAZ_00240051">
        <obo:RO_0001025 rdf:resource="http://purl.obolibrary.org/obo/GAZ_00239977"/>
        <obo:IAO_0000115>A suburb (neighborhood) of Cape Town.</obo:IAO_0000115>
        <oboInOwl:hasOBONamespace>GAZ</oboInOwl:hasOBONamespace>
        <oboInOwl:id>GAZ:00240051</oboInOwl:id>
        <rdfs:label>Sun Valley</rdfs:label>
    </owl:NamedIndividual>
    


    <!-- http://purl.obolibrary.org/obo/GAZ_00240053 -->

    <owl:NamedIndividual rdf:about="http://purl.obolibrary.org/obo/GAZ_00240053">
        <obo:RO_0001025 rdf:resource="http://purl.obolibrary.org/obo/GAZ_00076275"/>
        <obo:RO_0001025 rdf:resource="http://purl.obolibrary.org/obo/GAZ_00240048"/>
        <obo:IAO_0000115>A sheltered beach made up of inlets between granite boulders.</obo:IAO_0000115>
        <oboInOwl:hasOBONamespace>GAZ</oboInOwl:hasOBONamespace>
        <oboInOwl:id>GAZ:00240053</oboInOwl:id>
        <rdfs:label>Boulders Beach</rdfs:label>
    </owl:NamedIndividual>
    


    <!-- http://purl.obolibrary.org/obo/GAZ_00240054 -->

    <owl:NamedIndividual rdf:about="http://purl.obolibrary.org/obo/GAZ_00240054">
        <obo:RO_0001025 rdf:resource="http://purl.obolibrary.org/obo/GAZ_00239974"/>
        <obo:IAO_0000115>A suburb (neighborhood) of Cape Town.</obo:IAO_0000115>
        <oboInOwl:hasOBONamespace>GAZ</oboInOwl:hasOBONamespace>
        <oboInOwl:id>GAZ:00240054</oboInOwl:id>
        <rdfs:label>Bellville</rdfs:label>
    </owl:NamedIndividual>
    


    <!-- http://purl.obolibrary.org/obo/GAZ_00240055 -->

    <owl:NamedIndividual rdf:about="http://purl.obolibrary.org/obo/GAZ_00240055">
        <obo:RO_0001025 rdf:resource="http://purl.obolibrary.org/obo/GAZ_00239974"/>
        <obo:IAO_0000115>A suburb (neighborhood) of Cape Town.</obo:IAO_0000115>
        <oboInOwl:hasOBONamespace>GAZ</oboInOwl:hasOBONamespace>
        <oboInOwl:id>GAZ:00240055</oboInOwl:id>
        <rdfs:label>Bothasig</rdfs:label>
    </owl:NamedIndividual>
    


    <!-- http://purl.obolibrary.org/obo/GAZ_00240056 -->

    <owl:NamedIndividual rdf:about="http://purl.obolibrary.org/obo/GAZ_00240056">
        <obo:RO_0001025 rdf:resource="http://purl.obolibrary.org/obo/GAZ_00239974"/>
        <obo:IAO_0000115>A suburb (neighborhood) of Cape Town.</obo:IAO_0000115>
        <oboInOwl:hasOBONamespace>GAZ</oboInOwl:hasOBONamespace>
        <oboInOwl:id>GAZ:00240056</oboInOwl:id>
        <rdfs:label>Brackenfell</rdfs:label>
    </owl:NamedIndividual>
    


    <!-- http://purl.obolibrary.org/obo/GAZ_00240057 -->

    <owl:NamedIndividual rdf:about="http://purl.obolibrary.org/obo/GAZ_00240057">
        <obo:RO_0001025 rdf:resource="http://purl.obolibrary.org/obo/GAZ_00239974"/>
        <obo:IAO_0000115>A suburb (neighborhood) of Cape Town.</obo:IAO_0000115>
        <oboInOwl:hasOBONamespace>GAZ</oboInOwl:hasOBONamespace>
        <oboInOwl:id>GAZ:00240057</oboInOwl:id>
        <rdfs:label>Brooklyn</rdfs:label>
    </owl:NamedIndividual>
    


    <!-- http://purl.obolibrary.org/obo/GAZ_00240058 -->

    <owl:NamedIndividual rdf:about="http://purl.obolibrary.org/obo/GAZ_00240058">
        <obo:RO_0001025 rdf:resource="http://purl.obolibrary.org/obo/GAZ_00239974"/>
        <obo:IAO_0000115>A suburb (neighborhood) of Cape Town.</obo:IAO_0000115>
        <oboInOwl:hasOBONamespace>GAZ</oboInOwl:hasOBONamespace>
        <oboInOwl:id>GAZ:00240058</oboInOwl:id>
        <rdfs:label>Durbanville</rdfs:label>
    </owl:NamedIndividual>
    


    <!-- http://purl.obolibrary.org/obo/GAZ_00240059 -->

    <owl:NamedIndividual rdf:about="http://purl.obolibrary.org/obo/GAZ_00240059">
        <obo:RO_0001025 rdf:resource="http://purl.obolibrary.org/obo/GAZ_00239974"/>
        <obo:IAO_0000115>A suburb (neighborhood) of Cape Town.</obo:IAO_0000115>
        <oboInOwl:hasOBONamespace>GAZ</oboInOwl:hasOBONamespace>
        <oboInOwl:id>GAZ:00240059</oboInOwl:id>
        <rdfs:label>Edgemead</rdfs:label>
    </owl:NamedIndividual>
    


    <!-- http://purl.obolibrary.org/obo/GAZ_00240060 -->

    <owl:NamedIndividual rdf:about="http://purl.obolibrary.org/obo/GAZ_00240060">
        <obo:RO_0001025 rdf:resource="http://purl.obolibrary.org/obo/GAZ_00239973"/>
        <obo:IAO_0000115>A suburb (neighborhood) of Cape Town.</obo:IAO_0000115>
        <oboInOwl:hasOBONamespace>GAZ</oboInOwl:hasOBONamespace>
        <oboInOwl:id>GAZ:00240060</oboInOwl:id>
        <rdfs:label>Bo-Kaap</rdfs:label>
    </owl:NamedIndividual>
    


    <!-- http://purl.obolibrary.org/obo/GAZ_00240061 -->

    <owl:NamedIndividual rdf:about="http://purl.obolibrary.org/obo/GAZ_00240061">
        <obo:RO_0001025 rdf:resource="http://purl.obolibrary.org/obo/GAZ_00239974"/>
        <obo:IAO_0000115>A suburb (neighborhood) of Cape Town.</obo:IAO_0000115>
        <oboInOwl:hasOBONamespace>GAZ</oboInOwl:hasOBONamespace>
        <oboInOwl:id>GAZ:00240061</oboInOwl:id>
        <rdfs:label>Facreton</rdfs:label>
    </owl:NamedIndividual>
    


    <!-- http://purl.obolibrary.org/obo/GAZ_00240062 -->

    <owl:NamedIndividual rdf:about="http://purl.obolibrary.org/obo/GAZ_00240062">
        <obo:RO_0001025 rdf:resource="http://purl.obolibrary.org/obo/GAZ_00239974"/>
        <obo:IAO_0000115>A suburb (neighborhood) of Cape Town.</obo:IAO_0000115>
        <oboInOwl:hasOBONamespace>GAZ</oboInOwl:hasOBONamespace>
        <oboInOwl:id>GAZ:00240062</oboInOwl:id>
        <rdfs:label>Goodwood</rdfs:label>
    </owl:NamedIndividual>
    


    <!-- http://purl.obolibrary.org/obo/GAZ_00240063 -->

    <owl:NamedIndividual rdf:about="http://purl.obolibrary.org/obo/GAZ_00240063">
        <obo:RO_0001025 rdf:resource="http://purl.obolibrary.org/obo/GAZ_00239974"/>
        <obo:IAO_0000115>A suburb (neighborhood) of Cape Town.</obo:IAO_0000115>
        <oboInOwl:hasOBONamespace>GAZ</oboInOwl:hasOBONamespace>
        <oboInOwl:id>GAZ:00240063</oboInOwl:id>
        <rdfs:label>Kenridge</rdfs:label>
    </owl:NamedIndividual>
    


    <!-- http://purl.obolibrary.org/obo/GAZ_00240064 -->

    <owl:NamedIndividual rdf:about="http://purl.obolibrary.org/obo/GAZ_00240064">
        <obo:RO_0001025 rdf:resource="http://purl.obolibrary.org/obo/GAZ_00239974"/>
        <obo:IAO_0000115>A suburb (neighborhood) of Cape Town.</obo:IAO_0000115>
        <oboInOwl:hasOBONamespace>GAZ</oboInOwl:hasOBONamespace>
        <oboInOwl:id>GAZ:00240064</oboInOwl:id>
        <rdfs:label>Kensington</rdfs:label>
    </owl:NamedIndividual>
    


    <!-- http://purl.obolibrary.org/obo/GAZ_00240065 -->

    <owl:NamedIndividual rdf:about="http://purl.obolibrary.org/obo/GAZ_00240065">
        <obo:RO_0001025 rdf:resource="http://purl.obolibrary.org/obo/GAZ_00239974"/>
        <obo:IAO_0000115>A suburb (neighborhood) of Cape Town.</obo:IAO_0000115>
        <oboInOwl:hasOBONamespace>GAZ</oboInOwl:hasOBONamespace>
        <oboInOwl:id>GAZ:00240065</oboInOwl:id>
        <rdfs:label>Kuils River</rdfs:label>
    </owl:NamedIndividual>
    


    <!-- http://purl.obolibrary.org/obo/GAZ_00240066 -->

    <owl:NamedIndividual rdf:about="http://purl.obolibrary.org/obo/GAZ_00240066">
        <obo:RO_0001025 rdf:resource="http://purl.obolibrary.org/obo/GAZ_00239974"/>
        <obo:IAO_0000115>A suburb (neighborhood) of Cape Town.</obo:IAO_0000115>
        <oboInOwl:hasOBONamespace>GAZ</oboInOwl:hasOBONamespace>
        <oboInOwl:id>GAZ:00240066</oboInOwl:id>
        <rdfs:label>Maitland</rdfs:label>
    </owl:NamedIndividual>
    


    <!-- http://purl.obolibrary.org/obo/GAZ_00240067 -->

    <owl:NamedIndividual rdf:about="http://purl.obolibrary.org/obo/GAZ_00240067">
        <obo:RO_0001025 rdf:resource="http://purl.obolibrary.org/obo/GAZ_00239974"/>
        <obo:IAO_0000115>A suburb (neighborhood) of Cape Town.</obo:IAO_0000115>
        <oboInOwl:hasOBONamespace>GAZ</oboInOwl:hasOBONamespace>
        <oboInOwl:id>GAZ:00240067</oboInOwl:id>
        <rdfs:label>Monte Vista</rdfs:label>
    </owl:NamedIndividual>
    


    <!-- http://purl.obolibrary.org/obo/GAZ_00240068 -->

    <owl:NamedIndividual rdf:about="http://purl.obolibrary.org/obo/GAZ_00240068">
        <obo:RO_0001025 rdf:resource="http://purl.obolibrary.org/obo/GAZ_00239974"/>
        <obo:IAO_0000115>A suburb (neighborhood) of Cape Town.</obo:IAO_0000115>
        <oboInOwl:hasOBONamespace>GAZ</oboInOwl:hasOBONamespace>
        <oboInOwl:id>GAZ:00240068</oboInOwl:id>
        <rdfs:label>Panorama</rdfs:label>
    </owl:NamedIndividual>
    


    <!-- http://purl.obolibrary.org/obo/GAZ_00240069 -->

    <owl:NamedIndividual rdf:about="http://purl.obolibrary.org/obo/GAZ_00240069">
        <obo:RO_0001025 rdf:resource="http://purl.obolibrary.org/obo/GAZ_00239974"/>
        <obo:IAO_0000115>A suburb (neighborhood) of Cape Town.</obo:IAO_0000115>
        <oboInOwl:hasOBONamespace>GAZ</oboInOwl:hasOBONamespace>
        <oboInOwl:id>GAZ:00240069</oboInOwl:id>
        <rdfs:label>Parow</rdfs:label>
    </owl:NamedIndividual>
    


    <!-- http://purl.obolibrary.org/obo/GAZ_00240070 -->

    <owl:NamedIndividual rdf:about="http://purl.obolibrary.org/obo/GAZ_00240070">
        <obo:RO_0001025 rdf:resource="http://purl.obolibrary.org/obo/GAZ_00239974"/>
        <obo:IAO_0000115>A suburb (neighborhood) of Cape Town.</obo:IAO_0000115>
        <oboInOwl:hasOBONamespace>GAZ</oboInOwl:hasOBONamespace>
        <oboInOwl:id>GAZ:00240070</oboInOwl:id>
        <rdfs:label>Thornton</rdfs:label>
    </owl:NamedIndividual>
    


    <!-- http://purl.obolibrary.org/obo/GAZ_00240071 -->

    <owl:NamedIndividual rdf:about="http://purl.obolibrary.org/obo/GAZ_00240071">
        <obo:RO_0001025 rdf:resource="http://purl.obolibrary.org/obo/GAZ_00239973"/>
        <obo:IAO_0000115>A suburb (neighborhood) of Cape Town.</obo:IAO_0000115>
        <oboInOwl:hasOBONamespace>GAZ</oboInOwl:hasOBONamespace>
        <oboInOwl:id>GAZ:00240071</oboInOwl:id>
        <rdfs:label>De Waterkant</rdfs:label>
    </owl:NamedIndividual>
    


    <!-- http://purl.obolibrary.org/obo/GAZ_00240072 -->

    <owl:NamedIndividual rdf:about="http://purl.obolibrary.org/obo/GAZ_00240072">
        <obo:RO_0001025 rdf:resource="http://purl.obolibrary.org/obo/GAZ_00239974"/>
        <obo:IAO_0000115>A suburb (neighborhood) of Cape Town.</obo:IAO_0000115>
        <oboInOwl:hasOBONamespace>GAZ</oboInOwl:hasOBONamespace>
        <oboInOwl:id>GAZ:00240072</oboInOwl:id>
        <rdfs:label>Welgemoed</rdfs:label>
    </owl:NamedIndividual>
    


    <!-- http://purl.obolibrary.org/obo/GAZ_00240073 -->

    <owl:NamedIndividual rdf:about="http://purl.obolibrary.org/obo/GAZ_00240073">
        <obo:RO_0001025 rdf:resource="http://purl.obolibrary.org/obo/GAZ_00239973"/>
        <obo:IAO_0000115>A suburb (neighborhood) of Cape Town.</obo:IAO_0000115>
        <oboInOwl:hasOBONamespace>GAZ</oboInOwl:hasOBONamespace>
        <oboInOwl:id>GAZ:00240073</oboInOwl:id>
        <rdfs:label>Gardens</rdfs:label>
    </owl:NamedIndividual>
    


    <!-- http://purl.obolibrary.org/obo/GAZ_00240074 -->

    <owl:NamedIndividual rdf:about="http://purl.obolibrary.org/obo/GAZ_00240074">
        <obo:RO_0001025 rdf:resource="http://purl.obolibrary.org/obo/GAZ_00239973"/>
        <obo:IAO_0000115>A suburb (neighborhood) of Cape Town.</obo:IAO_0000115>
        <oboInOwl:hasOBONamespace>GAZ</oboInOwl:hasOBONamespace>
        <oboInOwl:id>GAZ:00240074</oboInOwl:id>
        <rdfs:label>Higgovale</rdfs:label>
    </owl:NamedIndividual>
    


    <!-- http://purl.obolibrary.org/obo/GAZ_00240075 -->

    <owl:NamedIndividual rdf:about="http://purl.obolibrary.org/obo/GAZ_00240075">
        <obo:RO_0001025 rdf:resource="http://purl.obolibrary.org/obo/GAZ_00239973"/>
        <obo:IAO_0000115>A suburb (neighborhood) of Cape Town.</obo:IAO_0000115>
        <oboInOwl:hasOBONamespace>GAZ</oboInOwl:hasOBONamespace>
        <oboInOwl:id>GAZ:00240075</oboInOwl:id>
        <rdfs:label>Oranjezicht</rdfs:label>
    </owl:NamedIndividual>
    


    <!-- http://purl.obolibrary.org/obo/GAZ_00240076 -->

    <owl:NamedIndividual rdf:about="http://purl.obolibrary.org/obo/GAZ_00240076">
        <obo:RO_0001025 rdf:resource="http://purl.obolibrary.org/obo/GAZ_00239973"/>
        <obo:IAO_0000115>A suburb (neighborhood) of Cape Town.</obo:IAO_0000115>
        <oboInOwl:hasOBONamespace>GAZ</oboInOwl:hasOBONamespace>
        <oboInOwl:id>GAZ:00240076</oboInOwl:id>
        <rdfs:label>Schotsche Kloof</rdfs:label>
    </owl:NamedIndividual>
    


    <!-- http://purl.obolibrary.org/obo/GAZ_00240077 -->

    <owl:NamedIndividual rdf:about="http://purl.obolibrary.org/obo/GAZ_00240077">
        <obo:RO_0001025 rdf:resource="http://purl.obolibrary.org/obo/GAZ_00239973"/>
        <obo:IAO_0000115>A suburb (neighborhood) of Cape Town.</obo:IAO_0000115>
        <oboInOwl:hasOBONamespace>GAZ</oboInOwl:hasOBONamespace>
        <oboInOwl:id>GAZ:00240077</oboInOwl:id>
        <rdfs:label>Tamboerskloof</rdfs:label>
    </owl:NamedIndividual>
    


    <!-- http://purl.obolibrary.org/obo/GAZ_00240078 -->

    <owl:NamedIndividual rdf:about="http://purl.obolibrary.org/obo/GAZ_00240078">
        <obo:RO_0001025 rdf:resource="http://purl.obolibrary.org/obo/GAZ_00239973"/>
        <obo:IAO_0000115>A suburb (neighborhood) of Cape Town.</obo:IAO_0000115>
        <oboInOwl:hasOBONamespace>GAZ</oboInOwl:hasOBONamespace>
        <oboInOwl:id>GAZ:00240078</oboInOwl:id>
        <rdfs:label>University Estate</rdfs:label>
    </owl:NamedIndividual>
    


    <!-- http://purl.obolibrary.org/obo/GAZ_00240079 -->

    <owl:NamedIndividual rdf:about="http://purl.obolibrary.org/obo/GAZ_00240079">
        <obo:RO_0001025 rdf:resource="http://purl.obolibrary.org/obo/GAZ_00239973"/>
        <obo:IAO_0000115>A suburb (neighborhood) of Cape Town.</obo:IAO_0000115>
        <oboInOwl:hasOBONamespace>GAZ</oboInOwl:hasOBONamespace>
        <oboInOwl:id>GAZ:00240079</oboInOwl:id>
        <rdfs:label>Vredehoek</rdfs:label>
    </owl:NamedIndividual>
    


    <!-- http://purl.obolibrary.org/obo/GAZ_00240080 -->

    <owl:NamedIndividual rdf:about="http://purl.obolibrary.org/obo/GAZ_00240080">
        <obo:RO_0001025 rdf:resource="http://purl.obolibrary.org/obo/GAZ_00239973"/>
        <obo:IAO_0000115>A suburb (neighborhood) of Cape Town.</obo:IAO_0000115>
        <oboInOwl:hasOBONamespace>GAZ</oboInOwl:hasOBONamespace>
        <oboInOwl:id>GAZ:00240080</oboInOwl:id>
        <rdfs:label>Walmer Estate</rdfs:label>
    </owl:NamedIndividual>
    


    <!-- http://purl.obolibrary.org/obo/GAZ_00240081 -->

    <owl:NamedIndividual rdf:about="http://purl.obolibrary.org/obo/GAZ_00240081">
        <obo:RO_0001025 rdf:resource="http://purl.obolibrary.org/obo/GAZ_00239973"/>
        <obo:IAO_0000115>A suburb (neighborhood) of Cape Town.</obo:IAO_0000115>
        <oboInOwl:hasOBONamespace>GAZ</oboInOwl:hasOBONamespace>
        <oboInOwl:id>GAZ:00240081</oboInOwl:id>
        <rdfs:label>Zonnebloem</rdfs:label>
    </owl:NamedIndividual>
    


    <!-- http://purl.obolibrary.org/obo/GAZ_00240082 -->

    <owl:NamedIndividual rdf:about="http://purl.obolibrary.org/obo/GAZ_00240082">
        <obo:RO_0001025 rdf:resource="http://purl.obolibrary.org/obo/GAZ_00239975"/>
        <obo:IAO_0000115>A suburb (neighborhood) of Cape Town.</obo:IAO_0000115>
        <oboInOwl:hasOBONamespace>GAZ</oboInOwl:hasOBONamespace>
        <oboInOwl:id>GAZ:00240082</oboInOwl:id>
        <rdfs:label>Bantry Bay</rdfs:label>
    </owl:NamedIndividual>
    


    <!-- http://purl.obolibrary.org/obo/GAZ_00240083 -->

    <owl:NamedIndividual rdf:about="http://purl.obolibrary.org/obo/GAZ_00240083">
        <obo:RO_0001025 rdf:resource="http://purl.obolibrary.org/obo/GAZ_00239975"/>
        <obo:IAO_0000115>A suburb (neighborhood) of Cape Town.</obo:IAO_0000115>
        <oboInOwl:hasOBONamespace>GAZ</oboInOwl:hasOBONamespace>
        <oboInOwl:id>GAZ:00240083</oboInOwl:id>
        <rdfs:label>Camps Bay</rdfs:label>
    </owl:NamedIndividual>
    


    <!-- http://purl.obolibrary.org/obo/GAZ_00240084 -->

    <owl:NamedIndividual rdf:about="http://purl.obolibrary.org/obo/GAZ_00240084">
        <obo:RO_0001025 rdf:resource="http://purl.obolibrary.org/obo/GAZ_00239975"/>
        <obo:IAO_0000115>A suburb (neighborhood) of Cape Town.</obo:IAO_0000115>
        <oboInOwl:hasOBONamespace>GAZ</oboInOwl:hasOBONamespace>
        <oboInOwl:id>GAZ:00240084</oboInOwl:id>
        <rdfs:label>Clifton</rdfs:label>
    </owl:NamedIndividual>
    


    <!-- http://purl.obolibrary.org/obo/GAZ_00240085 -->

    <owl:NamedIndividual rdf:about="http://purl.obolibrary.org/obo/GAZ_00240085">
        <obo:RO_0001025 rdf:resource="http://purl.obolibrary.org/obo/GAZ_00239975"/>
        <obo:IAO_0000115>A suburb (neighborhood) of Cape Town.</obo:IAO_0000115>
        <oboInOwl:hasOBONamespace>GAZ</oboInOwl:hasOBONamespace>
        <oboInOwl:id>GAZ:00240085</oboInOwl:id>
        <rdfs:label>Fresnaye</rdfs:label>
    </owl:NamedIndividual>
    


    <!-- http://purl.obolibrary.org/obo/GAZ_00240086 -->

    <owl:NamedIndividual rdf:about="http://purl.obolibrary.org/obo/GAZ_00240086">
        <obo:RO_0001025 rdf:resource="http://purl.obolibrary.org/obo/GAZ_00239975"/>
        <obo:IAO_0000115>A suburb (neighborhood) of Cape Town.</obo:IAO_0000115>
        <oboInOwl:hasOBONamespace>GAZ</oboInOwl:hasOBONamespace>
        <oboInOwl:id>GAZ:00240086</oboInOwl:id>
        <rdfs:label>Green Point</rdfs:label>
    </owl:NamedIndividual>
    


    <!-- http://purl.obolibrary.org/obo/GAZ_00240087 -->

    <owl:NamedIndividual rdf:about="http://purl.obolibrary.org/obo/GAZ_00240087">
        <obo:RO_0001025 rdf:resource="http://purl.obolibrary.org/obo/GAZ_00239975"/>
        <obo:IAO_0000115>A suburb (neighborhood) of Cape Town.</obo:IAO_0000115>
        <oboInOwl:hasOBONamespace>GAZ</oboInOwl:hasOBONamespace>
        <oboInOwl:id>GAZ:00240087</oboInOwl:id>
        <rdfs:label>Hout Bay</rdfs:label>
    </owl:NamedIndividual>
    


    <!-- http://purl.obolibrary.org/obo/GAZ_00240088 -->

    <owl:NamedIndividual rdf:about="http://purl.obolibrary.org/obo/GAZ_00240088">
        <obo:RO_0001025 rdf:resource="http://purl.obolibrary.org/obo/GAZ_00239975"/>
        <obo:IAO_0000115>A suburb (neighborhood) of Cape Town.</obo:IAO_0000115>
        <oboInOwl:hasOBONamespace>GAZ</oboInOwl:hasOBONamespace>
        <oboInOwl:id>GAZ:00240088</oboInOwl:id>
        <rdfs:label>Llandudno</rdfs:label>
    </owl:NamedIndividual>
    


    <!-- http://purl.obolibrary.org/obo/GAZ_00240089 -->

    <owl:NamedIndividual rdf:about="http://purl.obolibrary.org/obo/GAZ_00240089">
        <obo:RO_0001025 rdf:resource="http://purl.obolibrary.org/obo/GAZ_00239975"/>
        <obo:IAO_0000115>A suburb (neighborhood) of Cape Town.</obo:IAO_0000115>
        <oboInOwl:hasOBONamespace>GAZ</oboInOwl:hasOBONamespace>
        <oboInOwl:id>GAZ:00240089</oboInOwl:id>
        <rdfs:label>Mouille Point</rdfs:label>
    </owl:NamedIndividual>
    


    <!-- http://purl.obolibrary.org/obo/GAZ_00240090 -->

    <owl:NamedIndividual rdf:about="http://purl.obolibrary.org/obo/GAZ_00240090">
        <obo:RO_0001025 rdf:resource="http://purl.obolibrary.org/obo/GAZ_00239975"/>
        <obo:IAO_0000115>A suburb (neighborhood) of Cape Town.</obo:IAO_0000115>
        <oboInOwl:hasOBONamespace>GAZ</oboInOwl:hasOBONamespace>
        <oboInOwl:id>GAZ:00240090</oboInOwl:id>
        <rdfs:label>Sea Point</rdfs:label>
    </owl:NamedIndividual>
    


    <!-- http://purl.obolibrary.org/obo/GAZ_00240091 -->

    <owl:NamedIndividual rdf:about="http://purl.obolibrary.org/obo/GAZ_00240091">
        <obo:RO_0001025 rdf:resource="http://purl.obolibrary.org/obo/GAZ_00239975"/>
        <obo:IAO_0000115>A suburb (neighborhood) of Cape Town.</obo:IAO_0000115>
        <oboInOwl:hasOBONamespace>GAZ</oboInOwl:hasOBONamespace>
        <oboInOwl:id>GAZ:00240091</oboInOwl:id>
        <rdfs:label>Three Anchor Bay</rdfs:label>
    </owl:NamedIndividual>
    


    <!-- http://purl.obolibrary.org/obo/GAZ_00240092 -->

    <owl:NamedIndividual rdf:about="http://purl.obolibrary.org/obo/GAZ_00240092">
        <obo:RO_0001025 rdf:resource="http://purl.obolibrary.org/obo/GAZ_00032856"/>
        <obo:IAO_0000115>A protected area. It lies some 200km north of Cape Town, stretching from the Middelberg Pass at Citrusdal to north of the Pakhuis Pass at Clanwilliam. Established 1973.</obo:IAO_0000115>
        <oboInOwl:hasOBONamespace>GAZ</oboInOwl:hasOBONamespace>
        <oboInOwl:id>GAZ:00240092</oboInOwl:id>
        <rdfs:label>Cederberg Wilderness Area</rdfs:label>
    </owl:NamedIndividual>
    


    <!-- http://purl.obolibrary.org/obo/GAZ_00240093 -->

    <owl:NamedIndividual rdf:about="http://purl.obolibrary.org/obo/GAZ_00240093">
        <obo:RO_0001025 rdf:resource="http://purl.obolibrary.org/obo/GAZ_00032856"/>
        <obo:IAO_0000115>A protected area.</obo:IAO_0000115>
        <oboInOwl:hasOBONamespace>GAZ</oboInOwl:hasOBONamespace>
        <oboInOwl:id>GAZ:00240093</oboInOwl:id>
        <rdfs:label>Matjiesrivier Nature Reserve</rdfs:label>
    </owl:NamedIndividual>
    


    <!-- http://purl.obolibrary.org/obo/GAZ_00240094 -->

    <owl:NamedIndividual rdf:about="http://purl.obolibrary.org/obo/GAZ_00240094">
        <obo:RO_0001025 rdf:resource="http://purl.obolibrary.org/obo/GAZ_00032856"/>
        <obo:IAO_0000115>A bay.</obo:IAO_0000115>
        <oboInOwl:hasOBONamespace>GAZ</oboInOwl:hasOBONamespace>
        <oboInOwl:id>GAZ:00240094</oboInOwl:id>
        <rdfs:label>Lambert&apos;s Bay</rdfs:label>
    </owl:NamedIndividual>
    


    <!-- http://purl.obolibrary.org/obo/GAZ_00240095 -->

    <owl:NamedIndividual rdf:about="http://purl.obolibrary.org/obo/GAZ_00240095">
        <obo:RO_0001025 rdf:resource="http://purl.obolibrary.org/obo/GAZ_00240094"/>
        <obo:IAO_0000115>An island. It lies about 100 m off-shore of Lambert&apos;s Bay on the Cape west coast. Connected to the mainland by a breakwater in 1959.</obo:IAO_0000115>
        <oboInOwl:hasOBONamespace>GAZ</oboInOwl:hasOBONamespace>
        <oboInOwl:id>GAZ:00240095</oboInOwl:id>
        <rdfs:label>Bird Island</rdfs:label>
    </owl:NamedIndividual>
    


    <!-- http://purl.obolibrary.org/obo/GAZ_00240096 -->

    <owl:NamedIndividual rdf:about="http://purl.obolibrary.org/obo/GAZ_00240096">
        <obo:RO_0001025 rdf:resource="http://purl.obolibrary.org/obo/GAZ_00240095"/>
        <obo:IAO_0000115>A protected area.</obo:IAO_0000115>
        <oboInOwl:hasOBONamespace>GAZ</oboInOwl:hasOBONamespace>
        <oboInOwl:id>GAZ:00240096</oboInOwl:id>
        <rdfs:label>Bird Island Nature Reserve</rdfs:label>
    </owl:NamedIndividual>
    


    <!-- http://purl.obolibrary.org/obo/GAZ_00240097 -->

    <owl:NamedIndividual rdf:about="http://purl.obolibrary.org/obo/GAZ_00240097">
        <obo:RO_0001025 rdf:resource="http://purl.obolibrary.org/obo/GAZ_00032856"/>
        <obo:IAO_0000115>A protected area. Located 25 km north of Velddrif. Established 1988.</obo:IAO_0000115>
        <oboInOwl:hasOBONamespace>GAZ</oboInOwl:hasOBONamespace>
        <oboInOwl:id>GAZ:00240097</oboInOwl:id>
        <rdfs:label>Rocherpan Nature Reserve</rdfs:label>
    </owl:NamedIndividual>
    


    <!-- http://purl.obolibrary.org/obo/GAZ_00240098 -->

    <owl:NamedIndividual rdf:about="http://purl.obolibrary.org/obo/GAZ_00240098">
        <obo:RO_0001025 rdf:resource="http://purl.obolibrary.org/obo/GAZ_00032856"/>
        <obo:RO_0001025 rdf:resource="http://purl.obolibrary.org/obo/GAZ_00076141"/>
        <obo:IAO_0000115>A protected area.</obo:IAO_0000115>
        <oboInOwl:hasOBONamespace>GAZ</oboInOwl:hasOBONamespace>
        <oboInOwl:id>GAZ:00240098</oboInOwl:id>
        <rdfs:label>Groot Winterhoek Wilderness Area</rdfs:label>
    </owl:NamedIndividual>
    


    <!-- http://purl.obolibrary.org/obo/GAZ_00240099 -->

    <owl:NamedIndividual rdf:about="http://purl.obolibrary.org/obo/GAZ_00240099">
        <obo:RO_0001025 rdf:resource="http://purl.obolibrary.org/obo/GAZ_00012790"/>
        <obo:IAO_0000115>A reservoir. Located NW of Grabouw.</obo:IAO_0000115>
        <oboInOwl:hasOBONamespace>GAZ</oboInOwl:hasOBONamespace>
        <oboInOwl:id>GAZ:00240099</oboInOwl:id>
        <rdfs:label>Theewaterskloof Dam Reservoir</rdfs:label>
    </owl:NamedIndividual>
    


    <!-- http://purl.obolibrary.org/obo/GAZ_00240100 -->

    <owl:NamedIndividual rdf:about="http://purl.obolibrary.org/obo/GAZ_00240100">
        <obo:RO_0001025 rdf:resource="http://purl.obolibrary.org/obo/GAZ_00012790"/>
        <obo:RO_0001025 rdf:resource="http://purl.obolibrary.org/obo/GAZ_00076144"/>
        <obo:IAO_0000115>A protected area. Located in the Du Toitskloof mountains near Paarl, forming a part of the greater Boland mountain range.</obo:IAO_0000115>
        <oboInOwl:hasOBONamespace>GAZ</oboInOwl:hasOBONamespace>
        <oboInOwl:id>GAZ:00240100</oboInOwl:id>
        <rdfs:label>Limietberg Nature Reserve</rdfs:label>
    </owl:NamedIndividual>
    


    <!-- http://purl.obolibrary.org/obo/GAZ_00240101 -->

    <owl:NamedIndividual rdf:about="http://purl.obolibrary.org/obo/GAZ_00240101">
        <obo:RO_0001025 rdf:resource="http://purl.obolibrary.org/obo/GAZ_00012790"/>
        <obo:IAO_0000115>A protected area. Located near Stellenbosch in the south-western Cape.</obo:IAO_0000115>
        <oboInOwl:hasOBONamespace>GAZ</oboInOwl:hasOBONamespace>
        <oboInOwl:id>GAZ:00240101</oboInOwl:id>
        <rdfs:label>Jonkershoek Nature Reserve</rdfs:label>
    </owl:NamedIndividual>
    


    <!-- http://purl.obolibrary.org/obo/GAZ_00240102 -->

    <owl:NamedIndividual rdf:about="http://purl.obolibrary.org/obo/GAZ_00240102">
        <obo:RO_0001025 rdf:resource="http://purl.obolibrary.org/obo/GAZ_00012790"/>
        <obo:IAO_0000115>A protected area. Located approximately 9 km from Stellenbosch in the Jonkershoek Valley. It lies adjacent to the Eerste River which forms the northern boundary and extends up the north eastern slope of Stellenbosch Mountain which forms the southern boundary.</obo:IAO_0000115>
        <oboInOwl:hasOBONamespace>GAZ</oboInOwl:hasOBONamespace>
        <oboInOwl:id>GAZ:00240102</oboInOwl:id>
        <rdfs:label>Assegaaibosch Nature Reserve</rdfs:label>
    </owl:NamedIndividual>
    


    <!-- http://purl.obolibrary.org/obo/GAZ_00240104 -->

    <owl:NamedIndividual rdf:about="http://purl.obolibrary.org/obo/GAZ_00240104">
        <obo:RO_0001025 rdf:resource="http://purl.obolibrary.org/obo/GAZ_00005314"/>
        <obo:IAO_0000115>A suburb of Stellenbosch.</obo:IAO_0000115>
        <oboInOwl:hasOBONamespace>GAZ</oboInOwl:hasOBONamespace>
        <oboInOwl:id>GAZ:00240104</oboInOwl:id>
        <rdfs:label>Arbeidslus</rdfs:label>
    </owl:NamedIndividual>
    


    <!-- http://purl.obolibrary.org/obo/GAZ_00240105 -->

    <owl:NamedIndividual rdf:about="http://purl.obolibrary.org/obo/GAZ_00240105">
        <obo:RO_0001025 rdf:resource="http://purl.obolibrary.org/obo/GAZ_00005314"/>
        <obo:IAO_0000115>A suburb of Stellenbosch.</obo:IAO_0000115>
        <oboInOwl:hasOBONamespace>GAZ</oboInOwl:hasOBONamespace>
        <oboInOwl:id>GAZ:00240105</oboInOwl:id>
        <rdfs:label>Brandwag</rdfs:label>
    </owl:NamedIndividual>
    


    <!-- http://purl.obolibrary.org/obo/GAZ_00240106 -->

    <owl:NamedIndividual rdf:about="http://purl.obolibrary.org/obo/GAZ_00240106">
        <obo:RO_0001025 rdf:resource="http://purl.obolibrary.org/obo/GAZ_00005314"/>
        <obo:IAO_0000115>A suburb of Stellenbosch.</obo:IAO_0000115>
        <oboInOwl:hasOBONamespace>GAZ</oboInOwl:hasOBONamespace>
        <oboInOwl:id>GAZ:00240106</oboInOwl:id>
        <rdfs:label>Cloetesville</rdfs:label>
    </owl:NamedIndividual>
    


    <!-- http://purl.obolibrary.org/obo/GAZ_00240107 -->

    <owl:NamedIndividual rdf:about="http://purl.obolibrary.org/obo/GAZ_00240107">
        <obo:RO_0001025 rdf:resource="http://purl.obolibrary.org/obo/GAZ_00005314"/>
        <obo:IAO_0000115>A suburb of Stellenbosch.</obo:IAO_0000115>
        <oboInOwl:hasOBONamespace>GAZ</oboInOwl:hasOBONamespace>
        <oboInOwl:id>GAZ:00240107</oboInOwl:id>
        <rdfs:label>Dalsig</rdfs:label>
    </owl:NamedIndividual>
    


    <!-- http://purl.obolibrary.org/obo/GAZ_00240108 -->

    <owl:NamedIndividual rdf:about="http://purl.obolibrary.org/obo/GAZ_00240108">
        <obo:RO_0001025 rdf:resource="http://purl.obolibrary.org/obo/GAZ_00005314"/>
        <obo:IAO_0000115>A suburb of Stellenbosch.</obo:IAO_0000115>
        <oboInOwl:hasOBONamespace>GAZ</oboInOwl:hasOBONamespace>
        <oboInOwl:id>GAZ:00240108</oboInOwl:id>
        <rdfs:label>De Zalze</rdfs:label>
    </owl:NamedIndividual>
    


    <!-- http://purl.obolibrary.org/obo/GAZ_00240109 -->

    <owl:NamedIndividual rdf:about="http://purl.obolibrary.org/obo/GAZ_00240109">
        <obo:RO_0001025 rdf:resource="http://purl.obolibrary.org/obo/GAZ_00005314"/>
        <obo:IAO_0000115>A suburb of Stellenbosch.</obo:IAO_0000115>
        <oboInOwl:hasOBONamespace>GAZ</oboInOwl:hasOBONamespace>
        <oboInOwl:id>GAZ:00240109</oboInOwl:id>
        <rdfs:label>Dennesig</rdfs:label>
    </owl:NamedIndividual>
    


    <!-- http://purl.obolibrary.org/obo/GAZ_00240110 -->

    <owl:NamedIndividual rdf:about="http://purl.obolibrary.org/obo/GAZ_00240110">
        <obo:RO_0001025 rdf:resource="http://purl.obolibrary.org/obo/GAZ_00005314"/>
        <obo:IAO_0000115>A suburb of Stellenbosch.</obo:IAO_0000115>
        <oboInOwl:hasOBONamespace>GAZ</oboInOwl:hasOBONamespace>
        <oboInOwl:id>GAZ:00240110</oboInOwl:id>
        <rdfs:label>Die Boord</rdfs:label>
    </owl:NamedIndividual>
    


    <!-- http://purl.obolibrary.org/obo/GAZ_00240111 -->

    <owl:NamedIndividual rdf:about="http://purl.obolibrary.org/obo/GAZ_00240111">
        <obo:RO_0001025 rdf:resource="http://purl.obolibrary.org/obo/GAZ_00005314"/>
        <obo:IAO_0000115>A suburb of Stellenbosch.</obo:IAO_0000115>
        <oboInOwl:hasOBONamespace>GAZ</oboInOwl:hasOBONamespace>
        <oboInOwl:id>GAZ:00240111</oboInOwl:id>
        <rdfs:label>Die Rant</rdfs:label>
    </owl:NamedIndividual>
    


    <!-- http://purl.obolibrary.org/obo/GAZ_00240112 -->

    <owl:NamedIndividual rdf:about="http://purl.obolibrary.org/obo/GAZ_00240112">
        <obo:RO_0001025 rdf:resource="http://purl.obolibrary.org/obo/GAZ_00005314"/>
        <obo:IAO_0000115>A suburb of Stellenbosch.</obo:IAO_0000115>
        <oboInOwl:hasOBONamespace>GAZ</oboInOwl:hasOBONamespace>
        <oboInOwl:id>GAZ:00240112</oboInOwl:id>
        <rdfs:label>Idas Valley</rdfs:label>
    </owl:NamedIndividual>
    


    <!-- http://purl.obolibrary.org/obo/GAZ_00240113 -->

    <owl:NamedIndividual rdf:about="http://purl.obolibrary.org/obo/GAZ_00240113">
        <obo:RO_0001025 rdf:resource="http://purl.obolibrary.org/obo/GAZ_00005314"/>
        <obo:IAO_0000115>A suburb of Stellenbosch.</obo:IAO_0000115>
        <oboInOwl:hasOBONamespace>GAZ</oboInOwl:hasOBONamespace>
        <oboInOwl:id>GAZ:00240113</oboInOwl:id>
        <rdfs:label>Jamestown</rdfs:label>
    </owl:NamedIndividual>
    


    <!-- http://purl.obolibrary.org/obo/GAZ_00240114 -->

    <owl:NamedIndividual rdf:about="http://purl.obolibrary.org/obo/GAZ_00240114">
        <obo:RO_0001025 rdf:resource="http://purl.obolibrary.org/obo/GAZ_00005314"/>
        <obo:IAO_0000115>A suburb of Stellenbosch.</obo:IAO_0000115>
        <oboInOwl:hasOBONamespace>GAZ</oboInOwl:hasOBONamespace>
        <oboInOwl:id>GAZ:00240114</oboInOwl:id>
        <rdfs:label>Karindal</rdfs:label>
    </owl:NamedIndividual>
    


    <!-- http://purl.obolibrary.org/obo/GAZ_00240115 -->

    <owl:NamedIndividual rdf:about="http://purl.obolibrary.org/obo/GAZ_00240115">
        <obo:RO_0001025 rdf:resource="http://purl.obolibrary.org/obo/GAZ_00005314"/>
        <obo:IAO_0000115>A suburb of Stellenbosch.</obo:IAO_0000115>
        <oboInOwl:hasOBONamespace>GAZ</oboInOwl:hasOBONamespace>
        <oboInOwl:id>GAZ:00240115</oboInOwl:id>
        <rdfs:label>Krigeville</rdfs:label>
    </owl:NamedIndividual>
    


    <!-- http://purl.obolibrary.org/obo/GAZ_00240116 -->

    <owl:NamedIndividual rdf:about="http://purl.obolibrary.org/obo/GAZ_00240116">
        <obo:RO_0001025 rdf:resource="http://purl.obolibrary.org/obo/GAZ_00005314"/>
        <obo:IAO_0000115>A suburb of Stellenbosch.</obo:IAO_0000115>
        <oboInOwl:hasOBONamespace>GAZ</oboInOwl:hasOBONamespace>
        <oboInOwl:id>GAZ:00240116</oboInOwl:id>
        <rdfs:label>Kayamandi</rdfs:label>
    </owl:NamedIndividual>
    


    <!-- http://purl.obolibrary.org/obo/GAZ_00240117 -->

    <owl:NamedIndividual rdf:about="http://purl.obolibrary.org/obo/GAZ_00240117">
        <obo:RO_0001025 rdf:resource="http://purl.obolibrary.org/obo/GAZ_00005314"/>
        <obo:IAO_0000115>A suburb of Stellenbosch.</obo:IAO_0000115>
        <oboInOwl:hasOBONamespace>GAZ</oboInOwl:hasOBONamespace>
        <oboInOwl:id>GAZ:00240117</oboInOwl:id>
        <rdfs:label>Kylemore</rdfs:label>
    </owl:NamedIndividual>
    


    <!-- http://purl.obolibrary.org/obo/GAZ_00240118 -->

    <owl:NamedIndividual rdf:about="http://purl.obolibrary.org/obo/GAZ_00240118">
        <obo:RO_0001025 rdf:resource="http://purl.obolibrary.org/obo/GAZ_00005314"/>
        <obo:IAO_0000115>A suburb of Stellenbosch.</obo:IAO_0000115>
        <oboInOwl:hasOBONamespace>GAZ</oboInOwl:hasOBONamespace>
        <oboInOwl:id>GAZ:00240118</oboInOwl:id>
        <rdfs:label>Welbedaght</rdfs:label>
    </owl:NamedIndividual>
    


    <!-- http://purl.obolibrary.org/obo/GAZ_00240119 -->

    <owl:NamedIndividual rdf:about="http://purl.obolibrary.org/obo/GAZ_00240119">
        <obo:RO_0001025 rdf:resource="http://purl.obolibrary.org/obo/GAZ_00005314"/>
        <obo:IAO_0000115>A suburb of Stellenbosch.</obo:IAO_0000115>
        <oboInOwl:hasOBONamespace>GAZ</oboInOwl:hasOBONamespace>
        <oboInOwl:id>GAZ:00240119</oboInOwl:id>
        <rdfs:label>La Colline</rdfs:label>
    </owl:NamedIndividual>
    


    <!-- http://purl.obolibrary.org/obo/GAZ_00240120 -->

    <owl:NamedIndividual rdf:about="http://purl.obolibrary.org/obo/GAZ_00240120">
        <obo:RO_0001025 rdf:resource="http://purl.obolibrary.org/obo/GAZ_00005314"/>
        <obo:IAO_0000115>A suburb of Stellenbosch.</obo:IAO_0000115>
        <oboInOwl:hasOBONamespace>GAZ</oboInOwl:hasOBONamespace>
        <oboInOwl:id>GAZ:00240120</oboInOwl:id>
        <rdfs:label>Mostertsdrift</rdfs:label>
    </owl:NamedIndividual>
    


    <!-- http://purl.obolibrary.org/obo/GAZ_00240121 -->

    <owl:NamedIndividual rdf:about="http://purl.obolibrary.org/obo/GAZ_00240121">
        <obo:RO_0001025 rdf:resource="http://purl.obolibrary.org/obo/GAZ_00005314"/>
        <obo:IAO_0000115>A suburb of Stellenbosch.</obo:IAO_0000115>
        <oboInOwl:hasOBONamespace>GAZ</oboInOwl:hasOBONamespace>
        <oboInOwl:id>GAZ:00240121</oboInOwl:id>
        <rdfs:label>Onderpapegaaiberg</rdfs:label>
    </owl:NamedIndividual>
    


    <!-- http://purl.obolibrary.org/obo/GAZ_00240122 -->

    <owl:NamedIndividual rdf:about="http://purl.obolibrary.org/obo/GAZ_00240122">
        <obo:RO_0001025 rdf:resource="http://purl.obolibrary.org/obo/GAZ_00005314"/>
        <obo:IAO_0000115>A suburb of Stellenbosch.</obo:IAO_0000115>
        <oboInOwl:hasOBONamespace>GAZ</oboInOwl:hasOBONamespace>
        <oboInOwl:id>GAZ:00240122</oboInOwl:id>
        <rdfs:label>Paradyskloof</rdfs:label>
    </owl:NamedIndividual>
    


    <!-- http://purl.obolibrary.org/obo/GAZ_00240123 -->

    <owl:NamedIndividual rdf:about="http://purl.obolibrary.org/obo/GAZ_00240123">
        <obo:RO_0001025 rdf:resource="http://purl.obolibrary.org/obo/GAZ_00005314"/>
        <obo:IAO_0000115>A suburb of Stellenbosch.</obo:IAO_0000115>
        <oboInOwl:hasOBONamespace>GAZ</oboInOwl:hasOBONamespace>
        <oboInOwl:id>GAZ:00240123</oboInOwl:id>
        <rdfs:label>Plankenberg</rdfs:label>
    </owl:NamedIndividual>
    


    <!-- http://purl.obolibrary.org/obo/GAZ_00240124 -->

    <owl:NamedIndividual rdf:about="http://purl.obolibrary.org/obo/GAZ_00240124">
        <obo:RO_0001025 rdf:resource="http://purl.obolibrary.org/obo/GAZ_00005314"/>
        <obo:IAO_0000115>A suburb of Stellenbosch.</obo:IAO_0000115>
        <oboInOwl:hasOBONamespace>GAZ</oboInOwl:hasOBONamespace>
        <oboInOwl:id>GAZ:00240124</oboInOwl:id>
        <rdfs:label>Rozendal</rdfs:label>
    </owl:NamedIndividual>
    


    <!-- http://purl.obolibrary.org/obo/GAZ_00240125 -->

    <owl:NamedIndividual rdf:about="http://purl.obolibrary.org/obo/GAZ_00240125">
        <obo:RO_0001025 rdf:resource="http://purl.obolibrary.org/obo/GAZ_00005314"/>
        <obo:IAO_0000115>A suburb of Stellenbosch.</obo:IAO_0000115>
        <oboInOwl:hasOBONamespace>GAZ</oboInOwl:hasOBONamespace>
        <oboInOwl:id>GAZ:00240125</oboInOwl:id>
        <rdfs:label>Simonswyk</rdfs:label>
    </owl:NamedIndividual>
    


    <!-- http://purl.obolibrary.org/obo/GAZ_00240126 -->

    <owl:NamedIndividual rdf:about="http://purl.obolibrary.org/obo/GAZ_00240126">
        <obo:RO_0001025 rdf:resource="http://purl.obolibrary.org/obo/GAZ_00005314"/>
        <obo:IAO_0000115>A suburb of Stellenbosch.</obo:IAO_0000115>
        <oboInOwl:hasOBONamespace>GAZ</oboInOwl:hasOBONamespace>
        <oboInOwl:id>GAZ:00240126</oboInOwl:id>
        <rdfs:label>Techno Park</rdfs:label>
    </owl:NamedIndividual>
    


    <!-- http://purl.obolibrary.org/obo/GAZ_00240127 -->

    <owl:NamedIndividual rdf:about="http://purl.obolibrary.org/obo/GAZ_00240127">
        <obo:RO_0001025 rdf:resource="http://purl.obolibrary.org/obo/GAZ_00005314"/>
        <obo:IAO_0000115>A suburb of Stellenbosch.</obo:IAO_0000115>
        <oboInOwl:hasOBONamespace>GAZ</oboInOwl:hasOBONamespace>
        <oboInOwl:id>GAZ:00240127</oboInOwl:id>
        <rdfs:label>Tennantville</rdfs:label>
    </owl:NamedIndividual>
    


    <!-- http://purl.obolibrary.org/obo/GAZ_00240128 -->

    <owl:NamedIndividual rdf:about="http://purl.obolibrary.org/obo/GAZ_00240128">
        <obo:RO_0001025 rdf:resource="http://purl.obolibrary.org/obo/GAZ_00005314"/>
        <obo:IAO_0000115>A suburb of Stellenbosch.</obo:IAO_0000115>
        <oboInOwl:hasOBONamespace>GAZ</oboInOwl:hasOBONamespace>
        <oboInOwl:id>GAZ:00240128</oboInOwl:id>
        <rdfs:label>Town Central</rdfs:label>
    </owl:NamedIndividual>
    


    <!-- http://purl.obolibrary.org/obo/GAZ_00240129 -->

    <owl:NamedIndividual rdf:about="http://purl.obolibrary.org/obo/GAZ_00240129">
        <obo:RO_0001025 rdf:resource="http://purl.obolibrary.org/obo/GAZ_00005314"/>
        <obo:IAO_0000115>A suburb of Stellenbosch.</obo:IAO_0000115>
        <oboInOwl:hasOBONamespace>GAZ</oboInOwl:hasOBONamespace>
        <oboInOwl:id>GAZ:00240129</oboInOwl:id>
        <rdfs:label>Uniepark</rdfs:label>
    </owl:NamedIndividual>
    


    <!-- http://purl.obolibrary.org/obo/GAZ_00240130 -->

    <owl:NamedIndividual rdf:about="http://purl.obolibrary.org/obo/GAZ_00240130">
        <obo:RO_0001025 rdf:resource="http://purl.obolibrary.org/obo/GAZ_00005314"/>
        <obo:IAO_0000115>A suburb of Stellenbosch.</obo:IAO_0000115>
        <oboInOwl:hasOBONamespace>GAZ</oboInOwl:hasOBONamespace>
        <oboInOwl:id>GAZ:00240130</oboInOwl:id>
        <rdfs:label>Universiteitsoord</rdfs:label>
    </owl:NamedIndividual>
    


    <!-- http://purl.obolibrary.org/obo/GAZ_00240131 -->

    <owl:NamedIndividual rdf:about="http://purl.obolibrary.org/obo/GAZ_00240131">
        <obo:RO_0001025 rdf:resource="http://purl.obolibrary.org/obo/GAZ_00005314"/>
        <obo:IAO_0000115>A suburb of Stellenbosch.</obo:IAO_0000115>
        <oboInOwl:hasOBONamespace>GAZ</oboInOwl:hasOBONamespace>
        <oboInOwl:id>GAZ:00240131</oboInOwl:id>
        <rdfs:label>Welgevonden</rdfs:label>
    </owl:NamedIndividual>
    


    <!-- http://purl.obolibrary.org/obo/GAZ_00240132 -->

    <owl:NamedIndividual rdf:about="http://purl.obolibrary.org/obo/GAZ_00240132">
        <obo:RO_0001025 rdf:resource="http://purl.obolibrary.org/obo/GAZ_00032845"/>
        <obo:RO_0001025 rdf:resource="http://purl.obolibrary.org/obo/GAZ_00076151"/>
        <obo:IAO_0000115>A protected area. Located about 22 km northwest of Heidelberg.</obo:IAO_0000115>
        <oboInOwl:hasOBONamespace>GAZ</oboInOwl:hasOBONamespace>
        <oboInOwl:id>GAZ:00240132</oboInOwl:id>
        <rdfs:label>Grootvadersbosch Nature Reserve</rdfs:label>
    </owl:NamedIndividual>
    


    <!-- http://purl.obolibrary.org/obo/GAZ_00240134 -->

    <owl:NamedIndividual rdf:about="http://purl.obolibrary.org/obo/GAZ_00240134">
        <obo:RO_0001025 rdf:resource="http://purl.obolibrary.org/obo/GAZ_00032845"/>
        <obo:IAO_0000115>A protected area. Located 6 km south-east of Bredasdorp on the south-western Cape coast. The reserve lies at the mouth of the Heuningnes River, between the coastal villages of Arniston (Waenhuiskrans) and Struisbaai. Established 1986.</obo:IAO_0000115>
        <oboInOwl:hasOBONamespace>GAZ</oboInOwl:hasOBONamespace>
        <oboInOwl:id>GAZ:00240134</oboInOwl:id>
        <rdfs:label>De Mond Nature Reserve</rdfs:label>
    </owl:NamedIndividual>
    


    <!-- http://purl.obolibrary.org/obo/GAZ_00240136 -->

    <owl:NamedIndividual rdf:about="http://purl.obolibrary.org/obo/GAZ_00240136">
        <obo:RO_0001025 rdf:resource="http://purl.obolibrary.org/obo/GAZ_00076281"/>
        <obo:IAO_0000115>A reservoir.</obo:IAO_0000115>
        <oboInOwl:hasOBONamespace>GAZ</oboInOwl:hasOBONamespace>
        <oboInOwl:id>GAZ:00240136</oboInOwl:id>
        <rdfs:label>Wildebeesdam Reservoir</rdfs:label>
    </owl:NamedIndividual>
    


    <!-- http://purl.obolibrary.org/obo/GAZ_00240137 -->

    <owl:NamedIndividual rdf:about="http://purl.obolibrary.org/obo/GAZ_00240137">
        <obo:RO_0001025 rdf:resource="http://purl.obolibrary.org/obo/GAZ_00032845"/>
        <obo:IAO_0000115>A protected area. Located on the south-western Cape coast, just east of Hermanus. It comprises five coastal areas lying between Hermanus and Die Dam near Struisbaai. The largest area, known as Walker Bay, stretches from the Klein River estuary to De Kelders at Gansbaai.</obo:IAO_0000115>
        <oboInOwl:hasOBONamespace>GAZ</oboInOwl:hasOBONamespace>
        <oboInOwl:id>GAZ:00240137</oboInOwl:id>
        <rdfs:label>Walker Bay Nature Reserve</rdfs:label>
    </owl:NamedIndividual>
    


    <!-- http://purl.obolibrary.org/obo/GAZ_00240139 -->

    <owl:NamedIndividual rdf:about="http://purl.obolibrary.org/obo/GAZ_00240139">
        <obo:IAO_0000115>A lagoon at the mouth of the Klein River.</obo:IAO_0000115>
        <oboInOwl:hasOBONamespace>GAZ</oboInOwl:hasOBONamespace>
        <oboInOwl:id>GAZ:00240139</oboInOwl:id>
        <rdfs:label>Klein River Lagoon</rdfs:label>
    </owl:NamedIndividual>
    


    <!-- http://purl.obolibrary.org/obo/GAZ_00240140 -->

    <owl:NamedIndividual rdf:about="http://purl.obolibrary.org/obo/GAZ_00240140">
        <obo:RO_0001025 rdf:resource="http://purl.obolibrary.org/obo/GAZ_00032845"/>
        <obo:RO_0001025 rdf:resource="http://purl.obolibrary.org/obo/GAZ_00076136"/>
        <obo:IAO_0000115>A protected area. Established 1987.</obo:IAO_0000115>
        <oboInOwl:hasOBONamespace>GAZ</oboInOwl:hasOBONamespace>
        <oboInOwl:id>GAZ:00240140</oboInOwl:id>
        <rdfs:label>Kogelberg Nature Reserve</rdfs:label>
    </owl:NamedIndividual>
    


    <!-- http://purl.obolibrary.org/obo/GAZ_00240142 -->

    <owl:NamedIndividual rdf:about="http://purl.obolibrary.org/obo/GAZ_00240142">
        <obo:IAO_0000115>A reservoir.</obo:IAO_0000115>
        <oboInOwl:hasOBONamespace>GAZ</oboInOwl:hasOBONamespace>
        <oboInOwl:id>GAZ:00240142</oboInOwl:id>
        <rdfs:label>Buffelsrivierdam</rdfs:label>
    </owl:NamedIndividual>
    


    <!-- http://purl.obolibrary.org/obo/GAZ_00240143 -->

    <owl:NamedIndividual rdf:about="http://purl.obolibrary.org/obo/GAZ_00240143">
        <obo:RO_0001025 rdf:resource="http://purl.obolibrary.org/obo/GAZ_00032845"/>
        <obo:IAO_0000115>A bay.</obo:IAO_0000115>
        <oboInOwl:hasOBONamespace>GAZ</oboInOwl:hasOBONamespace>
        <oboInOwl:id>GAZ:00240143</oboInOwl:id>
        <rdfs:label>Pringle Bay</rdfs:label>
    </owl:NamedIndividual>
    


    <!-- http://purl.obolibrary.org/obo/GAZ_00240144 -->

    <owl:NamedIndividual rdf:about="http://purl.obolibrary.org/obo/GAZ_00240144">
        <obo:RO_0001025 rdf:resource="http://purl.obolibrary.org/obo/GAZ_00240140"/>
        <obo:IAO_0000115>A river. Discharges to the Atlantic Ocean.</obo:IAO_0000115>
        <oboInOwl:hasOBONamespace>GAZ</oboInOwl:hasOBONamespace>
        <oboInOwl:id>GAZ:00240144</oboInOwl:id>
        <rdfs:label>Rooielsrivier</rdfs:label>
    </owl:NamedIndividual>
    


    <!-- http://purl.obolibrary.org/obo/GAZ_00240145 -->

    <owl:NamedIndividual rdf:about="http://purl.obolibrary.org/obo/GAZ_00240145">
        <obo:RO_0001025 rdf:resource="http://purl.obolibrary.org/obo/GAZ_00032845"/>
        <obo:IAO_0000115>A river. Discharges to the Atlantic Ocean.</obo:IAO_0000115>
        <oboInOwl:hasOBONamespace>GAZ</oboInOwl:hasOBONamespace>
        <oboInOwl:id>GAZ:00240145</oboInOwl:id>
        <rdfs:label>Botrivier</rdfs:label>
    </owl:NamedIndividual>
    


    <!-- http://purl.obolibrary.org/obo/GAZ_00240146 -->

    <owl:NamedIndividual rdf:about="http://purl.obolibrary.org/obo/GAZ_00240146">
        <obo:RO_0001025 rdf:resource="http://purl.obolibrary.org/obo/GAZ_00240145"/>
        <obo:IAO_0000115>A lagoon at the estuary of the Botrivier.</obo:IAO_0000115>
        <oboInOwl:hasOBONamespace>GAZ</oboInOwl:hasOBONamespace>
        <oboInOwl:id>GAZ:00240146</oboInOwl:id>
        <rdfs:label>Botrivierviei</rdfs:label>
    </owl:NamedIndividual>
    


    <!-- http://purl.obolibrary.org/obo/GAZ_00240147 -->

    <owl:NamedIndividual rdf:about="http://purl.obolibrary.org/obo/GAZ_00240147">
        <obo:RO_0001025 rdf:resource="http://purl.obolibrary.org/obo/GAZ_00032845"/>
        <obo:IAO_0000115>A protected area. Borders the Botrivierviei.</obo:IAO_0000115>
        <oboInOwl:hasOBONamespace>GAZ</oboInOwl:hasOBONamespace>
        <oboInOwl:id>GAZ:00240147</oboInOwl:id>
        <rdfs:label>Rooisand Nature Reserve</rdfs:label>
    </owl:NamedIndividual>
    


    <!-- http://purl.obolibrary.org/obo/GAZ_00240148 -->

    <owl:NamedIndividual rdf:about="http://purl.obolibrary.org/obo/GAZ_00240148">
        <obo:RO_0001025 rdf:resource="http://purl.obolibrary.org/obo/GAZ_00032855"/>
        <obo:IAO_0000115>A protected area. Located in the Klein Karoo between Ladismith, Laingsburg, Touwsrivier and Montagu. Established 1988.</obo:IAO_0000115>
        <oboInOwl:hasOBONamespace>GAZ</oboInOwl:hasOBONamespace>
        <oboInOwl:id>GAZ:00240148</oboInOwl:id>
        <rdfs:label>Anysberg Nature Reserve</rdfs:label>
    </owl:NamedIndividual>
    


    <!-- http://purl.obolibrary.org/obo/GAZ_00240149 -->

    <owl:NamedIndividual rdf:about="http://purl.obolibrary.org/obo/GAZ_00240149">
        <obo:RO_0001025 rdf:resource="http://purl.obolibrary.org/obo/GAZ_00076120"/>
        <obo:IAO_0000115>A protected area.</obo:IAO_0000115>
        <oboInOwl:hasOBONamespace>GAZ</oboInOwl:hasOBONamespace>
        <oboInOwl:id>GAZ:00240149</oboInOwl:id>
        <rdfs:label>Gamkapoort Nature Reserve</rdfs:label>
    </owl:NamedIndividual>
    


    <!-- http://purl.obolibrary.org/obo/GAZ_00240150 -->

    <owl:NamedIndividual rdf:about="http://purl.obolibrary.org/obo/GAZ_00240150">
        <obo:RO_0001025 rdf:resource="http://purl.obolibrary.org/obo/GAZ_00076120"/>
        <obo:IAO_0000115>A protected area.</obo:IAO_0000115>
        <oboInOwl:hasOBONamespace>GAZ</oboInOwl:hasOBONamespace>
        <oboInOwl:id>GAZ:00240150</oboInOwl:id>
        <rdfs:label>Towerkop Nature Reserve</rdfs:label>
    </owl:NamedIndividual>
    


    <!-- http://purl.obolibrary.org/obo/GAZ_00240151 -->

    <owl:NamedIndividual rdf:about="http://purl.obolibrary.org/obo/GAZ_00240151">
        <obo:RO_0001025 rdf:resource="http://purl.obolibrary.org/obo/GAZ_00012792"/>
        <obo:RO_0001025 rdf:resource="http://purl.obolibrary.org/obo/GAZ_00076162"/>
        <obo:IAO_0000115>A protected area. Located near the town of George.</obo:IAO_0000115>
        <oboInOwl:hasOBONamespace>GAZ</oboInOwl:hasOBONamespace>
        <oboInOwl:id>GAZ:00240151</oboInOwl:id>
        <rdfs:label>Outeniqua Nature Reserve</rdfs:label>
    </owl:NamedIndividual>
    


    <!-- http://purl.obolibrary.org/obo/GAZ_00240152 -->

    <owl:NamedIndividual rdf:about="http://purl.obolibrary.org/obo/GAZ_00240152">
        <obo:RO_0001025 rdf:resource="http://purl.obolibrary.org/obo/GAZ_00012792"/>
        <obo:IAO_0000115>A protected area. Located approximately 40 km east of George and 20 km west of Knysna.</obo:IAO_0000115>
        <oboInOwl:hasOBONamespace>GAZ</oboInOwl:hasOBONamespace>
        <oboInOwl:id>GAZ:00240152</oboInOwl:id>
        <rdfs:label>Goukamma Nature Reserve</rdfs:label>
    </owl:NamedIndividual>
    


    <!-- http://purl.obolibrary.org/obo/GAZ_00240153 -->

    <owl:NamedIndividual rdf:about="http://purl.obolibrary.org/obo/GAZ_00240153">
        <obo:RO_0001025 rdf:resource="http://purl.obolibrary.org/obo/GAZ_00076131"/>
        <obo:IAO_0000115>A protected area.</obo:IAO_0000115>
        <oboInOwl:hasOBONamespace>GAZ</oboInOwl:hasOBONamespace>
        <oboInOwl:id>GAZ:00240153</oboInOwl:id>
        <rdfs:label>Keurbooms River Nature Reserve</rdfs:label>
    </owl:NamedIndividual>
    


    <!-- http://purl.obolibrary.org/obo/GAZ_00240154 -->

    <owl:NamedIndividual rdf:about="http://purl.obolibrary.org/obo/GAZ_00240154">
        <obo:RO_0001025 rdf:resource="http://purl.obolibrary.org/obo/GAZ_00240159"/>
        <obo:IAO_0000115>A protected area.</obo:IAO_0000115>
        <oboInOwl:hasOBONamespace>GAZ</oboInOwl:hasOBONamespace>
        <oboInOwl:id>GAZ:00240154</oboInOwl:id>
        <rdfs:label>Robberg Nature Reserve</rdfs:label>
    </owl:NamedIndividual>
    


    <!-- http://purl.obolibrary.org/obo/GAZ_00240155 -->

    <owl:NamedIndividual rdf:about="http://purl.obolibrary.org/obo/GAZ_00240155">
        <obo:RO_0001025 rdf:resource="http://purl.obolibrary.org/obo/GAZ_00012792"/>
        <obo:IAO_0000115>A protected area that extends for approximately 18 km from Buffalo Bay near to Sedgefield, and 1.8 km seaward.</obo:IAO_0000115>
        <oboInOwl:hasOBONamespace>GAZ</oboInOwl:hasOBONamespace>
        <oboInOwl:id>GAZ:00240155</oboInOwl:id>
        <rdfs:label>Goukamma Marine Protected Area</rdfs:label>
    </owl:NamedIndividual>
    


    <!-- http://purl.obolibrary.org/obo/GAZ_00240156 -->

    <owl:NamedIndividual rdf:about="http://purl.obolibrary.org/obo/GAZ_00240156">
        <obo:RO_0001025 rdf:resource="http://purl.obolibrary.org/obo/GAZ_00240152"/>
        <obo:IAO_0000115>A lake.</obo:IAO_0000115>
        <oboInOwl:hasOBONamespace>GAZ</oboInOwl:hasOBONamespace>
        <oboInOwl:id>GAZ:00240156</oboInOwl:id>
        <rdfs:label>Groenvlei</rdfs:label>
    </owl:NamedIndividual>
    


    <!-- http://purl.obolibrary.org/obo/GAZ_00240159 -->

    <owl:NamedIndividual rdf:about="http://purl.obolibrary.org/obo/GAZ_00240159">
        <obo:RO_0001025 rdf:resource="http://purl.obolibrary.org/obo/GAZ_00076131"/>
        <obo:IAO_0000115>A peninsula.</obo:IAO_0000115>
        <oboInOwl:hasOBONamespace>GAZ</oboInOwl:hasOBONamespace>
        <oboInOwl:id>GAZ:00240159</oboInOwl:id>
        <rdfs:label>Robberg</rdfs:label>
    </owl:NamedIndividual>
    


    <!-- http://purl.obolibrary.org/obo/GAZ_00240160 -->

    <owl:NamedIndividual rdf:about="http://purl.obolibrary.org/obo/GAZ_00240160">
        <obo:RO_0001025 rdf:resource="http://purl.obolibrary.org/obo/GAZ_00032845"/>
        <obo:IAO_0000115>A protected area extending 5 km to sea.</obo:IAO_0000115>
        <oboInOwl:hasOBONamespace>GAZ</oboInOwl:hasOBONamespace>
        <oboInOwl:id>GAZ:00240160</oboInOwl:id>
        <rdfs:label>De Hoop Marine Protected Area</rdfs:label>
    </owl:NamedIndividual>
    


    <!-- http://purl.obolibrary.org/obo/GAZ_00240161 -->

    <owl:NamedIndividual rdf:about="http://purl.obolibrary.org/obo/GAZ_00240161">
        <obo:RO_0001025 rdf:resource="http://purl.obolibrary.org/obo/GAZ_00012792"/>
        <obo:IAO_0000115>A protected area. Located near the town of Mossel Bay.</obo:IAO_0000115>
        <oboInOwl:hasOBONamespace>GAZ</oboInOwl:hasOBONamespace>
        <oboInOwl:id>GAZ:00240161</oboInOwl:id>
        <rdfs:label>Gondwana Game Reserve</rdfs:label>
    </owl:NamedIndividual>
    


    <!-- http://purl.obolibrary.org/obo/GAZ_00240164 -->

    <owl:NamedIndividual rdf:about="http://purl.obolibrary.org/obo/GAZ_00240164">
        <obo:RO_0001025 rdf:resource="http://purl.obolibrary.org/obo/GAZ_00002819"/>
        <obo:IAO_0000115>A river.</obo:IAO_0000115>
        <oboInOwl:hasOBONamespace>GAZ</oboInOwl:hasOBONamespace>
        <oboInOwl:id>GAZ:00240164</oboInOwl:id>
        <rdfs:label>Kraai River</rdfs:label>
    </owl:NamedIndividual>
    


    <!-- http://purl.obolibrary.org/obo/GAZ_00240165 -->

    <owl:NamedIndividual rdf:about="http://purl.obolibrary.org/obo/GAZ_00240165">
        <obo:RO_0001025 rdf:resource="http://purl.obolibrary.org/obo/GAZ_00002819"/>
        <obo:IAO_0000115>A river in South Africa which discharges into the Indian Ocean.</obo:IAO_0000115>
        <oboInOwl:hasOBONamespace>GAZ</oboInOwl:hasOBONamespace>
        <oboInOwl:id>GAZ:00240165</oboInOwl:id>
        <rdfs:label>Chalumna River</rdfs:label>
    </owl:NamedIndividual>
    


    <!-- http://purl.obolibrary.org/obo/GAZ_00240166 -->

    <owl:NamedIndividual rdf:about="http://purl.obolibrary.org/obo/GAZ_00240166">
        <obo:RO_0001025 rdf:resource="http://purl.obolibrary.org/obo/GAZ_00002819"/>
        <obo:IAO_0000115>A river running through the South African province of the Eastern Cape. Discharges to the Indin Ocean.</obo:IAO_0000115>
        <oboInOwl:hasOBONamespace>GAZ</oboInOwl:hasOBONamespace>
        <oboInOwl:id>GAZ:00240166</oboInOwl:id>
        <rdfs:label>Great Fish River</rdfs:label>
    </owl:NamedIndividual>
    


    <!-- http://purl.obolibrary.org/obo/GAZ_00240169 -->

    <owl:NamedIndividual rdf:about="http://purl.obolibrary.org/obo/GAZ_00240169">
        <obo:IAO_0000115>A headwater of Oliphants River.</obo:IAO_0000115>
        <oboInOwl:hasOBONamespace>GAZ</oboInOwl:hasOBONamespace>
        <oboInOwl:id>GAZ:00240169</oboInOwl:id>
        <rdfs:label>Traka River</rdfs:label>
    </owl:NamedIndividual>
    


    <!-- http://purl.obolibrary.org/obo/GAZ_00240170 -->

    <owl:NamedIndividual rdf:about="http://purl.obolibrary.org/obo/GAZ_00240170">
        <obo:IAO_0000115>A headwater of Oliphants River.</obo:IAO_0000115>
        <oboInOwl:hasOBONamespace>GAZ</oboInOwl:hasOBONamespace>
        <oboInOwl:id>GAZ:00240170</oboInOwl:id>
        <rdfs:label>Kalkwal River</rdfs:label>
    </owl:NamedIndividual>
    


    <!-- http://purl.obolibrary.org/obo/GAZ_00240172 -->

    <owl:NamedIndividual rdf:about="http://purl.obolibrary.org/obo/GAZ_00240172">
        <obo:RO_0001025 rdf:resource="http://purl.obolibrary.org/obo/GAZ_00002819"/>
        <obo:IAO_0000115>A river of Eastern Cape Province.</obo:IAO_0000115>
        <oboInOwl:hasOBONamespace>GAZ</oboInOwl:hasOBONamespace>
        <oboInOwl:id>GAZ:00240172</oboInOwl:id>
        <rdfs:label>Swartkops River</rdfs:label>
    </owl:NamedIndividual>
    


    <!-- http://purl.obolibrary.org/obo/GAZ_00240173 -->

    <owl:NamedIndividual rdf:about="http://purl.obolibrary.org/obo/GAZ_00240173">
        <obo:RO_0001025 rdf:resource="http://purl.obolibrary.org/obo/GAZ_00002819"/>
        <obo:IAO_0000115>A river of Eastern Cape Province.</obo:IAO_0000115>
        <oboInOwl:hasOBONamespace>GAZ</oboInOwl:hasOBONamespace>
        <oboInOwl:id>GAZ:00240173</oboInOwl:id>
        <rdfs:label>Mbashe River</rdfs:label>
    </owl:NamedIndividual>
    


    <!-- http://purl.obolibrary.org/obo/GAZ_00240174 -->

    <owl:NamedIndividual rdf:about="http://purl.obolibrary.org/obo/GAZ_00240174">
        <obo:RO_0001025 rdf:resource="http://purl.obolibrary.org/obo/GAZ_00002819"/>
        <obo:IAO_0000115>A river of Eastern Cape Province.</obo:IAO_0000115>
        <oboInOwl:hasOBONamespace>GAZ</oboInOwl:hasOBONamespace>
        <oboInOwl:id>GAZ:00240174</oboInOwl:id>
        <rdfs:label>Mzamba River</rdfs:label>
    </owl:NamedIndividual>
    


    <!-- http://purl.obolibrary.org/obo/GAZ_00240175 -->

    <owl:NamedIndividual rdf:about="http://purl.obolibrary.org/obo/GAZ_00240175">
        <obo:RO_0001025 rdf:resource="http://purl.obolibrary.org/obo/GAZ_00002819"/>
        <obo:IAO_0000115>A river of Eastern Cape Province.</obo:IAO_0000115>
        <oboInOwl:hasOBONamespace>GAZ</oboInOwl:hasOBONamespace>
        <oboInOwl:id>GAZ:00240175</oboInOwl:id>
        <rdfs:label>Mzimvubu River</rdfs:label>
    </owl:NamedIndividual>
    


    <!-- http://purl.obolibrary.org/obo/GAZ_00240176 -->

    <owl:NamedIndividual rdf:about="http://purl.obolibrary.org/obo/GAZ_00240176">
        <obo:RO_0001025 rdf:resource="http://purl.obolibrary.org/obo/GAZ_00002819"/>
        <obo:IAO_0000115>A river of Eastern Cape Province.</obo:IAO_0000115>
        <oboInOwl:hasOBONamespace>GAZ</oboInOwl:hasOBONamespace>
        <oboInOwl:id>GAZ:00240176</oboInOwl:id>
        <rdfs:label>Qolora River</rdfs:label>
    </owl:NamedIndividual>
    


    <!-- http://purl.obolibrary.org/obo/GAZ_00240177 -->

    <owl:NamedIndividual rdf:about="http://purl.obolibrary.org/obo/GAZ_00240177">
        <obo:RO_0001025 rdf:resource="http://purl.obolibrary.org/obo/GAZ_00002819"/>
        <obo:IAO_0000115>A river of Eastern Cape Province.</obo:IAO_0000115>
        <oboInOwl:hasOBONamespace>GAZ</oboInOwl:hasOBONamespace>
        <oboInOwl:id>GAZ:00240177</oboInOwl:id>
        <rdfs:label>Qora River</rdfs:label>
    </owl:NamedIndividual>
    


    <!-- http://purl.obolibrary.org/obo/GAZ_00240178 -->

    <owl:NamedIndividual rdf:about="http://purl.obolibrary.org/obo/GAZ_00240178">
        <obo:RO_0001025 rdf:resource="http://purl.obolibrary.org/obo/GAZ_00002819"/>
        <obo:IAO_0000115>A river of Eastern Cape Province.</obo:IAO_0000115>
        <oboInOwl:hasOBONamespace>GAZ</oboInOwl:hasOBONamespace>
        <oboInOwl:id>GAZ:00240178</oboInOwl:id>
        <rdfs:label>Klasies River</rdfs:label>
    </owl:NamedIndividual>
    


    <!-- http://purl.obolibrary.org/obo/GAZ_00240179 -->

    <owl:NamedIndividual rdf:about="http://purl.obolibrary.org/obo/GAZ_00240179">
        <obo:RO_0001025 rdf:resource="http://purl.obolibrary.org/obo/GAZ_00002819"/>
        <obo:IAO_0000115>A river of Eastern Cape Province.</obo:IAO_0000115>
        <oboInOwl:hasOBONamespace>GAZ</oboInOwl:hasOBONamespace>
        <oboInOwl:id>GAZ:00240179</oboInOwl:id>
        <rdfs:label>Xuka River</rdfs:label>
    </owl:NamedIndividual>
    


    <!-- http://purl.obolibrary.org/obo/GAZ_00240181 -->

    <owl:NamedIndividual rdf:about="http://purl.obolibrary.org/obo/GAZ_00240181">
        <obo:RO_0001025 rdf:resource="http://purl.obolibrary.org/obo/GAZ_00002819"/>
        <obo:IAO_0000115>A river of Eastern Cape Province.</obo:IAO_0000115>
        <oboInOwl:hasOBONamespace>GAZ</oboInOwl:hasOBONamespace>
        <oboInOwl:id>GAZ:00240181</oboInOwl:id>
        <rdfs:label>Rufanes River</rdfs:label>
    </owl:NamedIndividual>
    


    <!-- http://purl.obolibrary.org/obo/GAZ_00240182 -->

    <owl:NamedIndividual rdf:about="http://purl.obolibrary.org/obo/GAZ_00240182">
        <obo:RO_0001025 rdf:resource="http://purl.obolibrary.org/obo/GAZ_00002819"/>
        <obo:IAO_0000115>A river of Eastern Cape Province.</obo:IAO_0000115>
        <oboInOwl:hasOBONamespace>GAZ</oboInOwl:hasOBONamespace>
        <oboInOwl:id>GAZ:00240182</oboInOwl:id>
        <rdfs:label>Kaaimans River</rdfs:label>
    </owl:NamedIndividual>
    


    <!-- http://purl.obolibrary.org/obo/GAZ_00240183 -->

    <owl:NamedIndividual rdf:about="http://purl.obolibrary.org/obo/GAZ_00240183">
        <obo:RO_0001025 rdf:resource="http://purl.obolibrary.org/obo/GAZ_00002819"/>
        <obo:IAO_0000115>A river of Eastern Cape Province.</obo:IAO_0000115>
        <oboInOwl:hasOBONamespace>GAZ</oboInOwl:hasOBONamespace>
        <oboInOwl:id>GAZ:00240183</oboInOwl:id>
        <rdfs:label>Kammanassie River</rdfs:label>
    </owl:NamedIndividual>
    


    <!-- http://purl.obolibrary.org/obo/GAZ_00240184 -->

    <owl:NamedIndividual rdf:about="http://purl.obolibrary.org/obo/GAZ_00240184">
        <obo:RO_0001025 rdf:resource="http://purl.obolibrary.org/obo/GAZ_00002819"/>
        <obo:IAO_0000115>A river of Eastern Cape Province.</obo:IAO_0000115>
        <oboInOwl:hasOBONamespace>GAZ</oboInOwl:hasOBONamespace>
        <oboInOwl:id>GAZ:00240184</oboInOwl:id>
        <rdfs:label>Keiskamma River</rdfs:label>
    </owl:NamedIndividual>
    


    <!-- http://purl.obolibrary.org/obo/GAZ_00240185 -->

    <owl:NamedIndividual rdf:about="http://purl.obolibrary.org/obo/GAZ_00240185">
        <obo:RO_0001025 rdf:resource="http://purl.obolibrary.org/obo/GAZ_00002819"/>
        <obo:IAO_0000115>A river of Eastern Cape Province.</obo:IAO_0000115>
        <oboInOwl:hasOBONamespace>GAZ</oboInOwl:hasOBONamespace>
        <oboInOwl:id>GAZ:00240185</oboInOwl:id>
        <rdfs:label>Keurbooms River</rdfs:label>
    </owl:NamedIndividual>
    


    <!-- http://purl.obolibrary.org/obo/GAZ_00240186 -->

    <owl:NamedIndividual rdf:about="http://purl.obolibrary.org/obo/GAZ_00240186">
        <obo:IAO_0000115>A dam. Constructed 1973.</obo:IAO_0000115>
        <oboInOwl:hasOBONamespace>GAZ</oboInOwl:hasOBONamespace>
        <oboInOwl:id>GAZ:00240186</oboInOwl:id>
        <rdfs:label>Welbedacht Dam</rdfs:label>
    </owl:NamedIndividual>
    


    <!-- http://purl.obolibrary.org/obo/GAZ_00240187 -->

    <owl:NamedIndividual rdf:about="http://purl.obolibrary.org/obo/GAZ_00240187">
        <obo:RO_0001025 rdf:resource="http://purl.obolibrary.org/obo/GAZ_00002819"/>
        <obo:IAO_0000115>A river of Eastern Cape Province.</obo:IAO_0000115>
        <oboInOwl:hasOBONamespace>GAZ</oboInOwl:hasOBONamespace>
        <oboInOwl:id>GAZ:00240187</oboInOwl:id>
        <rdfs:label>Lyndoch River</rdfs:label>
    </owl:NamedIndividual>
    


    <!-- http://purl.obolibrary.org/obo/GAZ_00240188 -->

    <owl:NamedIndividual rdf:about="http://purl.obolibrary.org/obo/GAZ_00240188">
        <obo:RO_0001025 rdf:resource="http://purl.obolibrary.org/obo/GAZ_00002819"/>
        <obo:IAO_0000115>A river of Eastern Cape Province.</obo:IAO_0000115>
        <oboInOwl:hasOBONamespace>GAZ</oboInOwl:hasOBONamespace>
        <oboInOwl:id>GAZ:00240188</oboInOwl:id>
        <rdfs:label>Bushman River</rdfs:label>
    </owl:NamedIndividual>
    


    <!-- http://purl.obolibrary.org/obo/GAZ_00240189 -->

    <owl:NamedIndividual rdf:about="http://purl.obolibrary.org/obo/GAZ_00240189">
        <obo:RO_0001025 rdf:resource="http://purl.obolibrary.org/obo/GAZ_00002813"/>
        <obo:IAO_0000115>A river of Free State Province.</obo:IAO_0000115>
        <oboInOwl:hasOBONamespace>GAZ</oboInOwl:hasOBONamespace>
        <oboInOwl:id>GAZ:00240189</oboInOwl:id>
        <rdfs:label>Liebenbergsvlei River</rdfs:label>
    </owl:NamedIndividual>
    


    <!-- http://purl.obolibrary.org/obo/GAZ_00240190 -->

    <owl:NamedIndividual rdf:about="http://purl.obolibrary.org/obo/GAZ_00240190">
        <obo:RO_0001025 rdf:resource="http://purl.obolibrary.org/obo/GAZ_00002813"/>
        <obo:IAO_0000115>A river of Free State Province.</obo:IAO_0000115>
        <oboInOwl:hasOBONamespace>GAZ</oboInOwl:hasOBONamespace>
        <oboInOwl:id>GAZ:00240190</oboInOwl:id>
        <rdfs:label>Sand River</rdfs:label>
    </owl:NamedIndividual>
    


    <!-- http://purl.obolibrary.org/obo/GAZ_00240191 -->

    <owl:NamedIndividual rdf:about="http://purl.obolibrary.org/obo/GAZ_00240191">
        <obo:RO_0001025 rdf:resource="http://purl.obolibrary.org/obo/GAZ_00002813"/>
        <obo:IAO_0000115>A river of Free State Province.</obo:IAO_0000115>
        <oboInOwl:hasOBONamespace>GAZ</oboInOwl:hasOBONamespace>
        <oboInOwl:id>GAZ:00240191</oboInOwl:id>
        <rdfs:label>Vals River</rdfs:label>
    </owl:NamedIndividual>
    


    <!-- http://purl.obolibrary.org/obo/GAZ_00240192 -->

    <owl:NamedIndividual rdf:about="http://purl.obolibrary.org/obo/GAZ_00240192">
        <obo:RO_0001025 rdf:resource="http://purl.obolibrary.org/obo/GAZ_00002813"/>
        <obo:IAO_0000115>A river of Free State Province.</obo:IAO_0000115>
        <oboInOwl:hasOBONamespace>GAZ</oboInOwl:hasOBONamespace>
        <oboInOwl:id>GAZ:00240192</oboInOwl:id>
        <rdfs:label>Vet River</rdfs:label>
    </owl:NamedIndividual>
    


    <!-- http://purl.obolibrary.org/obo/GAZ_00240193 -->

    <owl:NamedIndividual rdf:about="http://purl.obolibrary.org/obo/GAZ_00240193">
        <obo:RO_0001025 rdf:resource="http://purl.obolibrary.org/obo/GAZ_00002813"/>
        <obo:IAO_0000115>A river of Free State Province.</obo:IAO_0000115>
        <oboInOwl:hasOBONamespace>GAZ</oboInOwl:hasOBONamespace>
        <oboInOwl:id>GAZ:00240193</oboInOwl:id>
        <rdfs:label>Wilge River</rdfs:label>
    </owl:NamedIndividual>
    


    <!-- http://purl.obolibrary.org/obo/GAZ_00240194 -->

    <owl:NamedIndividual rdf:about="http://purl.obolibrary.org/obo/GAZ_00240194">
        <obo:RO_0001025 rdf:resource="http://purl.obolibrary.org/obo/GAZ_00005318"/>
        <obo:IAO_0000115>A river.</obo:IAO_0000115>
        <oboInOwl:hasOBONamespace>GAZ</oboInOwl:hasOBONamespace>
        <oboInOwl:id>GAZ:00240194</oboInOwl:id>
        <rdfs:label>Jukskei River</rdfs:label>
    </owl:NamedIndividual>
    


    <!-- http://purl.obolibrary.org/obo/GAZ_00240195 -->

    <owl:NamedIndividual rdf:about="http://purl.obolibrary.org/obo/GAZ_00240195">
        <obo:RO_0001025 rdf:resource="http://purl.obolibrary.org/obo/GAZ_00005311"/>
        <obo:IAO_0000115>A river that flows through the city of Pretoria, South Africa. Its source is located just south of the city and it flows northward until it drains into the Pienaars River.</obo:IAO_0000115>
        <oboInOwl:hasOBONamespace>GAZ</oboInOwl:hasOBONamespace>
        <oboInOwl:id>GAZ:00240195</oboInOwl:id>
        <rdfs:label>Apies River</rdfs:label>
    </owl:NamedIndividual>
    


    <!-- http://purl.obolibrary.org/obo/GAZ_00240196 -->

    <owl:NamedIndividual rdf:about="http://purl.obolibrary.org/obo/GAZ_00240196">
        <obo:RO_0001025 rdf:resource="http://purl.obolibrary.org/obo/GAZ_00240195"/>
        <obo:IAO_0000115>A reservoir.</obo:IAO_0000115>
        <oboInOwl:hasOBONamespace>GAZ</oboInOwl:hasOBONamespace>
        <oboInOwl:id>GAZ:00240196</oboInOwl:id>
        <rdfs:label>Bon Accord Dam</rdfs:label>
    </owl:NamedIndividual>
    


    <!-- http://purl.obolibrary.org/obo/GAZ_00240197 -->

    <owl:NamedIndividual rdf:about="http://purl.obolibrary.org/obo/GAZ_00240197">
        <obo:RO_0001025 rdf:resource="http://purl.obolibrary.org/obo/GAZ_00002812"/>
        <obo:IAO_0000115>A river of KwaZulu-Natal Province.</obo:IAO_0000115>
        <oboInOwl:hasOBONamespace>GAZ</oboInOwl:hasOBONamespace>
        <oboInOwl:id>GAZ:00240197</oboInOwl:id>
        <rdfs:label>Mkomazi River</rdfs:label>
    </owl:NamedIndividual>
    


    <!-- http://purl.obolibrary.org/obo/GAZ_00240198 -->

    <owl:NamedIndividual rdf:about="http://purl.obolibrary.org/obo/GAZ_00240198">
        <obo:RO_0001025 rdf:resource="http://purl.obolibrary.org/obo/GAZ_00002812"/>
        <obo:IAO_0000115>A river of KwaZulu-Natal Province. It drains South Mosi Swamp.</obo:IAO_0000115>
        <oboInOwl:hasOBONamespace>GAZ</oboInOwl:hasOBONamespace>
        <oboInOwl:id>GAZ:00240198</oboInOwl:id>
        <rdfs:label>Mkuze River</rdfs:label>
    </owl:NamedIndividual>
    


    <!-- http://purl.obolibrary.org/obo/GAZ_00240199 -->

    <owl:NamedIndividual rdf:about="http://purl.obolibrary.org/obo/GAZ_00240199">
        <obo:RO_0001025 rdf:resource="http://purl.obolibrary.org/obo/GAZ_00002812"/>
        <obo:IAO_0000115>A river of KwaZulu-Natal Province.</obo:IAO_0000115>
        <oboInOwl:hasOBONamespace>GAZ</oboInOwl:hasOBONamespace>
        <oboInOwl:id>GAZ:00240199</oboInOwl:id>
        <rdfs:label>Mzumbe River</rdfs:label>
    </owl:NamedIndividual>
    


    <!-- http://purl.obolibrary.org/obo/GAZ_00240200 -->

    <owl:NamedIndividual rdf:about="http://purl.obolibrary.org/obo/GAZ_00240200">
        <obo:RO_0001025 rdf:resource="http://purl.obolibrary.org/obo/GAZ_00002812"/>
        <obo:IAO_0000115>A river of KwaZulu-Natal Province.</obo:IAO_0000115>
        <oboInOwl:hasOBONamespace>GAZ</oboInOwl:hasOBONamespace>
        <oboInOwl:id>GAZ:00240200</oboInOwl:id>
        <rdfs:label>Mlazi River</rdfs:label>
    </owl:NamedIndividual>
    


    <!-- http://purl.obolibrary.org/obo/GAZ_00240201 -->

    <owl:NamedIndividual rdf:about="http://purl.obolibrary.org/obo/GAZ_00240201">
        <obo:RO_0001025 rdf:resource="http://purl.obolibrary.org/obo/GAZ_00002812"/>
        <obo:IAO_0000115>A river of KwaZulu-Natal Province.</obo:IAO_0000115>
        <oboInOwl:hasOBONamespace>GAZ</oboInOwl:hasOBONamespace>
        <oboInOwl:id>GAZ:00240201</oboInOwl:id>
        <rdfs:label>Buffalo River</rdfs:label>
    </owl:NamedIndividual>
    


    <!-- http://purl.obolibrary.org/obo/GAZ_00240202 -->

    <owl:NamedIndividual rdf:about="http://purl.obolibrary.org/obo/GAZ_00240202">
        <obo:RO_0001025 rdf:resource="http://purl.obolibrary.org/obo/GAZ_00032881"/>
        <obo:IAO_0000115>A river in the Waterberg area of Limpopo Province, South Africa. This river&apos;s catchment basin is a sub-watershed of the Limpopo River. The river drains much of the Lapalala Wilderness area.</obo:IAO_0000115>
        <oboInOwl:hasOBONamespace>GAZ</oboInOwl:hasOBONamespace>
        <oboInOwl:id>GAZ:00240202</oboInOwl:id>
        <rdfs:label>Palala River</rdfs:label>
    </owl:NamedIndividual>
    


    <!-- http://purl.obolibrary.org/obo/GAZ_00240203 -->

    <owl:NamedIndividual rdf:about="http://purl.obolibrary.org/obo/GAZ_00240203">
        <obo:RO_0001025 rdf:resource="http://purl.obolibrary.org/obo/GAZ_00032881"/>
        <obo:IAO_0000115>A major watercourse in Limpopo Province of South Africa. This river collects much of the drainage of the Waterberg Massif and discharges it to the Limpopo River. It threads through the Waterberg Massif.</obo:IAO_0000115>
        <oboInOwl:hasOBONamespace>GAZ</oboInOwl:hasOBONamespace>
        <oboInOwl:id>GAZ:00240203</oboInOwl:id>
        <rdfs:label>Mokolo River</rdfs:label>
    </owl:NamedIndividual>
    


    <!-- http://purl.obolibrary.org/obo/GAZ_00240204 -->

    <owl:NamedIndividual rdf:about="http://purl.obolibrary.org/obo/GAZ_00240204">
        <obo:RO_0001025 rdf:resource="http://purl.obolibrary.org/obo/GAZ_00002814"/>
        <obo:IAO_0000115>A river of Limpopo Province.</obo:IAO_0000115>
        <oboInOwl:hasOBONamespace>GAZ</oboInOwl:hasOBONamespace>
        <oboInOwl:id>GAZ:00240204</oboInOwl:id>
        <rdfs:label>Levubu River</rdfs:label>
    </owl:NamedIndividual>
    


    <!-- http://purl.obolibrary.org/obo/GAZ_00240205 -->

    <owl:NamedIndividual rdf:about="http://purl.obolibrary.org/obo/GAZ_00240205">
        <obo:RO_0001025 rdf:resource="http://purl.obolibrary.org/obo/GAZ_00002814"/>
        <obo:IAO_0000115>A river of Limpopo Province.</obo:IAO_0000115>
        <oboInOwl:hasOBONamespace>GAZ</oboInOwl:hasOBONamespace>
        <oboInOwl:id>GAZ:00240205</oboInOwl:id>
        <rdfs:label>Letsitele River</rdfs:label>
    </owl:NamedIndividual>
    


    <!-- http://purl.obolibrary.org/obo/GAZ_00240206 -->

    <owl:NamedIndividual rdf:about="http://purl.obolibrary.org/obo/GAZ_00240206">
        <obo:RO_0001025 rdf:resource="http://purl.obolibrary.org/obo/GAZ_00002814"/>
        <obo:IAO_0000115>A river of Limpopo Province.</obo:IAO_0000115>
        <oboInOwl:hasOBONamespace>GAZ</oboInOwl:hasOBONamespace>
        <oboInOwl:id>GAZ:00240206</oboInOwl:id>
        <rdfs:label>Nyl River</rdfs:label>
    </owl:NamedIndividual>
    


    <!-- http://purl.obolibrary.org/obo/GAZ_00240207 -->

    <owl:NamedIndividual rdf:about="http://purl.obolibrary.org/obo/GAZ_00240207">
        <obo:RO_0001025 rdf:resource="http://purl.obolibrary.org/obo/GAZ_00002814"/>
        <obo:IAO_0000115>A river of Limpopo Province.</obo:IAO_0000115>
        <oboInOwl:hasOBONamespace>GAZ</oboInOwl:hasOBONamespace>
        <oboInOwl:id>GAZ:00240207</oboInOwl:id>
        <rdfs:label>Sand River</rdfs:label>
    </owl:NamedIndividual>
    


    <!-- http://purl.obolibrary.org/obo/GAZ_00240208 -->

    <owl:NamedIndividual rdf:about="http://purl.obolibrary.org/obo/GAZ_00240208">
        <obo:RO_0001025 rdf:resource="http://purl.obolibrary.org/obo/GAZ_00002814"/>
        <obo:IAO_0000115>A river of Limpopo Province.</obo:IAO_0000115>
        <oboInOwl:hasOBONamespace>GAZ</oboInOwl:hasOBONamespace>
        <oboInOwl:id>GAZ:00240208</oboInOwl:id>
        <rdfs:label>Shingwidzi River</rdfs:label>
    </owl:NamedIndividual>
    


    <!-- http://purl.obolibrary.org/obo/GAZ_00240210 -->

    <owl:NamedIndividual rdf:about="http://purl.obolibrary.org/obo/GAZ_00240210">
        <obo:RO_0001025 rdf:resource="http://purl.obolibrary.org/obo/GAZ_00002816"/>
        <obo:IAO_0000115>A river of Mpumalanga Province.</obo:IAO_0000115>
        <oboInOwl:hasOBONamespace>GAZ</oboInOwl:hasOBONamespace>
        <oboInOwl:id>GAZ:00240210</oboInOwl:id>
        <rdfs:label>Elands River</rdfs:label>
    </owl:NamedIndividual>
    


    <!-- http://purl.obolibrary.org/obo/GAZ_00240211 -->

    <owl:NamedIndividual rdf:about="http://purl.obolibrary.org/obo/GAZ_00240211">
        <obo:RO_0001025 rdf:resource="http://purl.obolibrary.org/obo/GAZ_00002816"/>
        <obo:IAO_0000115>A river of Mpumalanga Province.</obo:IAO_0000115>
        <oboInOwl:hasOBONamespace>GAZ</oboInOwl:hasOBONamespace>
        <oboInOwl:id>GAZ:00240211</oboInOwl:id>
        <rdfs:label>Emanzimhlope River</rdfs:label>
    </owl:NamedIndividual>
    


    <!-- http://purl.obolibrary.org/obo/GAZ_00240212 -->

    <owl:NamedIndividual rdf:about="http://purl.obolibrary.org/obo/GAZ_00240212">
        <obo:RO_0001025 rdf:resource="http://purl.obolibrary.org/obo/GAZ_00002816"/>
        <obo:IAO_0000115>A river of Mpumalanga Province.</obo:IAO_0000115>
        <oboInOwl:hasOBONamespace>GAZ</oboInOwl:hasOBONamespace>
        <oboInOwl:id>GAZ:00240212</oboInOwl:id>
        <rdfs:label>Lunsklip River</rdfs:label>
    </owl:NamedIndividual>
    


    <!-- http://purl.obolibrary.org/obo/GAZ_00240213 -->

    <owl:NamedIndividual rdf:about="http://purl.obolibrary.org/obo/GAZ_00240213">
        <obo:RO_0001025 rdf:resource="http://purl.obolibrary.org/obo/GAZ_00002818"/>
        <obo:IAO_0000115>A river.</obo:IAO_0000115>
        <oboInOwl:hasOBONamespace>GAZ</oboInOwl:hasOBONamespace>
        <oboInOwl:id>GAZ:00240213</oboInOwl:id>
        <rdfs:label>Sak River</rdfs:label>
    </owl:NamedIndividual>
    


    <!-- http://purl.obolibrary.org/obo/GAZ_00240215 -->

    <owl:NamedIndividual rdf:about="http://purl.obolibrary.org/obo/GAZ_00240215">
        <obo:RO_0001025 rdf:resource="http://purl.obolibrary.org/obo/GAZ_00009437"/>
        <obo:IAO_0000115>A river.</obo:IAO_0000115>
        <oboInOwl:hasOBONamespace>GAZ</oboInOwl:hasOBONamespace>
        <oboInOwl:id>GAZ:00240215</oboInOwl:id>
        <rdfs:label>Kuilsrivier</rdfs:label>
    </owl:NamedIndividual>
    


    <!-- http://purl.obolibrary.org/obo/GAZ_00240217 -->

    <owl:NamedIndividual rdf:about="http://purl.obolibrary.org/obo/GAZ_00240217">
        <obo:RO_0001025 rdf:resource="http://purl.obolibrary.org/obo/GAZ_00002817"/>
        <obo:IAO_0000115>A river of Western Cape Province.</obo:IAO_0000115>
        <oboInOwl:hasOBONamespace>GAZ</oboInOwl:hasOBONamespace>
        <oboInOwl:id>GAZ:00240217</oboInOwl:id>
        <rdfs:label>Lourens River</rdfs:label>
    </owl:NamedIndividual>
    


    <!-- http://purl.obolibrary.org/obo/GAZ_00240220 -->

    <owl:NamedIndividual rdf:about="http://purl.obolibrary.org/obo/GAZ_00240220">
        <obo:IAO_0000115>A dam.</obo:IAO_0000115>
        <oboInOwl:hasOBONamespace>GAZ</oboInOwl:hasOBONamespace>
        <oboInOwl:id>GAZ:00240220</oboInOwl:id>
        <rdfs:label>Newberry Dam</rdfs:label>
    </owl:NamedIndividual>
    


    <!-- http://purl.obolibrary.org/obo/GAZ_00240221 -->

    <owl:NamedIndividual rdf:about="http://purl.obolibrary.org/obo/GAZ_00240221">
        <obo:RO_0001025 rdf:resource="http://purl.obolibrary.org/obo/GAZ_00002819"/>
        <obo:IAO_0000115>A river.</obo:IAO_0000115>
        <oboInOwl:hasOBONamespace>GAZ</oboInOwl:hasOBONamespace>
        <oboInOwl:id>GAZ:00240221</oboInOwl:id>
        <rdfs:label>Kouga River</rdfs:label>
    </owl:NamedIndividual>
    


    <!-- http://purl.obolibrary.org/obo/GAZ_00240222 -->

    <owl:NamedIndividual rdf:about="http://purl.obolibrary.org/obo/GAZ_00240222">
        <obo:RO_0001025 rdf:resource="http://purl.obolibrary.org/obo/GAZ_00240221"/>
        <obo:IAO_0000115>A dam. Constructed 1967.</obo:IAO_0000115>
        <oboInOwl:hasOBONamespace>GAZ</oboInOwl:hasOBONamespace>
        <oboInOwl:id>GAZ:00240222</oboInOwl:id>
        <rdfs:label>Kouga Dam</rdfs:label>
    </owl:NamedIndividual>
    


    <!-- http://purl.obolibrary.org/obo/GAZ_00240223 -->

    <owl:NamedIndividual rdf:about="http://purl.obolibrary.org/obo/GAZ_00240223">
        <obo:RO_0001025 rdf:resource="http://purl.obolibrary.org/obo/GAZ_00240204"/>
        <obo:IAO_0000115>A dam. Located just outside the town of Louis Trichart Limpopo, is south of Musina. Constructed 1952.</obo:IAO_0000115>
        <oboInOwl:hasOBONamespace>GAZ</oboInOwl:hasOBONamespace>
        <oboInOwl:id>GAZ:00240223</oboInOwl:id>
        <rdfs:label>Albasini Dam</rdfs:label>
    </owl:NamedIndividual>
    


    <!-- http://purl.obolibrary.org/obo/GAZ_00240224 -->

    <owl:NamedIndividual rdf:about="http://purl.obolibrary.org/obo/GAZ_00240224">
        <obo:IAO_0000115>A dam.</obo:IAO_0000115>
        <oboInOwl:hasOBONamespace>GAZ</oboInOwl:hasOBONamespace>
        <oboInOwl:id>GAZ:00240224</oboInOwl:id>
        <rdfs:label>Berg River Dam</rdfs:label>
    </owl:NamedIndividual>
    


    <!-- http://purl.obolibrary.org/obo/GAZ_00240225 -->

    <owl:NamedIndividual rdf:about="http://purl.obolibrary.org/obo/GAZ_00240225">
        <obo:RO_0001025 rdf:resource="http://purl.obolibrary.org/obo/GAZ_00002816"/>
        <obo:IAO_0000115>A river.</obo:IAO_0000115>
        <oboInOwl:hasOBONamespace>GAZ</oboInOwl:hasOBONamespace>
        <oboInOwl:id>GAZ:00240225</oboInOwl:id>
        <rdfs:label>Assegaai River</rdfs:label>
    </owl:NamedIndividual>
    


    <!-- http://purl.obolibrary.org/obo/GAZ_00240226 -->

    <owl:NamedIndividual rdf:about="http://purl.obolibrary.org/obo/GAZ_00240226">
        <obo:RO_0001025 rdf:resource="http://purl.obolibrary.org/obo/GAZ_00240225"/>
        <obo:IAO_0000115>A dam.</obo:IAO_0000115>
        <oboInOwl:hasOBONamespace>GAZ</oboInOwl:hasOBONamespace>
        <oboInOwl:id>GAZ:00240226</oboInOwl:id>
        <rdfs:label>Heyshope Dam</rdfs:label>
    </owl:NamedIndividual>
    


    <!-- http://purl.obolibrary.org/obo/GAZ_00240227 -->

    <owl:NamedIndividual rdf:about="http://purl.obolibrary.org/obo/GAZ_00240227">
        <obo:IAO_0000115>A dam.</obo:IAO_0000115>
        <oboInOwl:hasOBONamespace>GAZ</oboInOwl:hasOBONamespace>
        <oboInOwl:id>GAZ:00240227</oboInOwl:id>
        <rdfs:label>BlydeRivierpoort Dam</rdfs:label>
    </owl:NamedIndividual>
    


    <!-- http://purl.obolibrary.org/obo/GAZ_00240228 -->

    <owl:NamedIndividual rdf:about="http://purl.obolibrary.org/obo/GAZ_00240228">
        <obo:IAO_0000115>A dam.</obo:IAO_0000115>
        <oboInOwl:hasOBONamespace>GAZ</oboInOwl:hasOBONamespace>
        <oboInOwl:id>GAZ:00240228</oboInOwl:id>
        <rdfs:label>Kwena Dam</rdfs:label>
    </owl:NamedIndividual>
    


    <!-- http://purl.obolibrary.org/obo/GAZ_00240229 -->

    <owl:NamedIndividual rdf:about="http://purl.obolibrary.org/obo/GAZ_00240229">
        <obo:RO_0001025 rdf:resource="http://purl.obolibrary.org/obo/GAZ_00239405"/>
        <obo:IAO_0000115>A dam.</obo:IAO_0000115>
        <oboInOwl:hasOBONamespace>GAZ</oboInOwl:hasOBONamespace>
        <oboInOwl:id>GAZ:00240229</oboInOwl:id>
        <rdfs:label>Driekoppies Dam</rdfs:label>
    </owl:NamedIndividual>
    


    <!-- http://purl.obolibrary.org/obo/GAZ_00240230 -->

    <owl:NamedIndividual rdf:about="http://purl.obolibrary.org/obo/GAZ_00240230">
        <obo:RO_0001025 rdf:resource="http://purl.obolibrary.org/obo/GAZ_00002816"/>
        <obo:IAO_0000115>A river.</obo:IAO_0000115>
        <oboInOwl:hasOBONamespace>GAZ</oboInOwl:hasOBONamespace>
        <oboInOwl:id>GAZ:00240230</oboInOwl:id>
        <rdfs:label>Marite River</rdfs:label>
    </owl:NamedIndividual>
    


    <!-- http://purl.obolibrary.org/obo/GAZ_00240231 -->

    <owl:NamedIndividual rdf:about="http://purl.obolibrary.org/obo/GAZ_00240231">
        <obo:RO_0001025 rdf:resource="http://purl.obolibrary.org/obo/GAZ_00240230"/>
        <obo:IAO_0000115>A dam.</obo:IAO_0000115>
        <oboInOwl:hasOBONamespace>GAZ</oboInOwl:hasOBONamespace>
        <oboInOwl:id>GAZ:00240231</oboInOwl:id>
        <rdfs:label>Inyaka Dam</rdfs:label>
    </owl:NamedIndividual>
    


    <!-- http://purl.obolibrary.org/obo/GAZ_00240232 -->

    <owl:NamedIndividual rdf:about="http://purl.obolibrary.org/obo/GAZ_00240232">
        <obo:RO_0001025 rdf:resource="http://purl.obolibrary.org/obo/GAZ_00002816"/>
        <obo:IAO_0000115>A river.</obo:IAO_0000115>
        <oboInOwl:hasOBONamespace>GAZ</oboInOwl:hasOBONamespace>
        <oboInOwl:id>GAZ:00240232</oboInOwl:id>
        <rdfs:label>Slang River</rdfs:label>
    </owl:NamedIndividual>
    


    <!-- http://purl.obolibrary.org/obo/GAZ_00240233 -->

    <owl:NamedIndividual rdf:about="http://purl.obolibrary.org/obo/GAZ_00240233">
        <obo:RO_0001025 rdf:resource="http://purl.obolibrary.org/obo/GAZ_00240232"/>
        <obo:IAO_0000115>A dam.</obo:IAO_0000115>
        <oboInOwl:hasOBONamespace>GAZ</oboInOwl:hasOBONamespace>
        <oboInOwl:id>GAZ:00240233</oboInOwl:id>
        <rdfs:label>Zaaihoek Dam</rdfs:label>
    </owl:NamedIndividual>
    


    <!-- http://purl.obolibrary.org/obo/GAZ_00240234 -->

    <owl:NamedIndividual rdf:about="http://purl.obolibrary.org/obo/GAZ_00240234">
        <obo:RO_0001025 rdf:resource="http://purl.obolibrary.org/obo/GAZ_00002816"/>
        <obo:IAO_0000115>A dam.</obo:IAO_0000115>
        <oboInOwl:hasOBONamespace>GAZ</oboInOwl:hasOBONamespace>
        <oboInOwl:id>GAZ:00240234</oboInOwl:id>
        <rdfs:label>Grootdraai Dam</rdfs:label>
    </owl:NamedIndividual>
    


    <!-- http://purl.obolibrary.org/obo/GAZ_00240235 -->

    <owl:NamedIndividual rdf:about="http://purl.obolibrary.org/obo/GAZ_00240235">
        <obo:RO_0001025 rdf:resource="http://purl.obolibrary.org/obo/GAZ_00002818"/>
        <obo:IAO_0000115>A river.</obo:IAO_0000115>
        <oboInOwl:hasOBONamespace>GAZ</oboInOwl:hasOBONamespace>
        <oboInOwl:id>GAZ:00240235</oboInOwl:id>
        <rdfs:label>Vanwyksvlei River</rdfs:label>
    </owl:NamedIndividual>
    


    <!-- http://purl.obolibrary.org/obo/GAZ_00240236 -->

    <owl:NamedIndividual rdf:about="http://purl.obolibrary.org/obo/GAZ_00240236">
        <obo:RO_0001025 rdf:resource="http://purl.obolibrary.org/obo/GAZ_00240235"/>
        <obo:IAO_0000115>A dam.</obo:IAO_0000115>
        <oboInOwl:hasOBONamespace>GAZ</oboInOwl:hasOBONamespace>
        <oboInOwl:id>GAZ:00240236</oboInOwl:id>
        <rdfs:label>Vanwyksvlei Dam</rdfs:label>
    </owl:NamedIndividual>
    


    <!-- http://purl.obolibrary.org/obo/GAZ_00240237 -->

    <owl:NamedIndividual rdf:about="http://purl.obolibrary.org/obo/GAZ_00240237">
        <obo:IAO_0000115>A dam.</obo:IAO_0000115>
        <oboInOwl:hasOBONamespace>GAZ</oboInOwl:hasOBONamespace>
        <oboInOwl:id>GAZ:00240237</oboInOwl:id>
        <rdfs:label>Teewaterskloof Dam</rdfs:label>
    </owl:NamedIndividual>
    


    <!-- http://purl.obolibrary.org/obo/GAZ_00240238 -->

    <owl:NamedIndividual rdf:about="http://purl.obolibrary.org/obo/GAZ_00240238">
        <obo:RO_0001025 rdf:resource="http://purl.obolibrary.org/obo/GAZ_00002817"/>
        <obo:IAO_0000115>A river.</obo:IAO_0000115>
        <oboInOwl:hasOBONamespace>GAZ</oboInOwl:hasOBONamespace>
        <oboInOwl:id>GAZ:00240238</oboInOwl:id>
        <rdfs:label>Voelvlei</rdfs:label>
    </owl:NamedIndividual>
    


    <!-- http://purl.obolibrary.org/obo/GAZ_00240239 -->

    <owl:NamedIndividual rdf:about="http://purl.obolibrary.org/obo/GAZ_00240239">
        <obo:RO_0001025 rdf:resource="http://purl.obolibrary.org/obo/GAZ_00240238"/>
        <obo:IAO_0000115>A dam.</obo:IAO_0000115>
        <oboInOwl:hasOBONamespace>GAZ</oboInOwl:hasOBONamespace>
        <oboInOwl:id>GAZ:00240239</oboInOwl:id>
        <rdfs:label>Voelvlei Dam</rdfs:label>
    </owl:NamedIndividual>
    


    <!-- http://purl.obolibrary.org/obo/GAZ_00240240 -->

    <owl:NamedIndividual rdf:about="http://purl.obolibrary.org/obo/GAZ_00240240">
        <obo:RO_0001025 rdf:resource="http://purl.obolibrary.org/obo/GAZ_00002817"/>
        <obo:IAO_0000115>A river.</obo:IAO_0000115>
        <oboInOwl:hasOBONamespace>GAZ</oboInOwl:hasOBONamespace>
        <oboInOwl:id>GAZ:00240240</oboInOwl:id>
        <rdfs:label>Waboomsrivier</rdfs:label>
    </owl:NamedIndividual>
    


    <!-- http://purl.obolibrary.org/obo/GAZ_00240241 -->

    <owl:NamedIndividual rdf:about="http://purl.obolibrary.org/obo/GAZ_00240241">
        <obo:RO_0001025 rdf:resource="http://purl.obolibrary.org/obo/GAZ_00240240"/>
        <obo:IAO_0000115>A dam.</obo:IAO_0000115>
        <oboInOwl:hasOBONamespace>GAZ</oboInOwl:hasOBONamespace>
        <oboInOwl:id>GAZ:00240241</oboInOwl:id>
        <rdfs:label>Kwaggaskloof Dam</rdfs:label>
    </owl:NamedIndividual>
    


    <!-- http://purl.obolibrary.org/obo/GAZ_00240242 -->

    <owl:NamedIndividual rdf:about="http://purl.obolibrary.org/obo/GAZ_00240242">
        <obo:RO_0001025 rdf:resource="http://purl.obolibrary.org/obo/GAZ_00002819"/>
        <obo:IAO_0000115>A river.</obo:IAO_0000115>
        <oboInOwl:hasOBONamespace>GAZ</oboInOwl:hasOBONamespace>
        <oboInOwl:id>GAZ:00240242</oboInOwl:id>
        <rdfs:label>Indwe River</rdfs:label>
    </owl:NamedIndividual>
    


    <!-- http://purl.obolibrary.org/obo/GAZ_00240243 -->

    <owl:NamedIndividual rdf:about="http://purl.obolibrary.org/obo/GAZ_00240243">
        <obo:RO_0001025 rdf:resource="http://purl.obolibrary.org/obo/GAZ_00240242"/>
        <obo:IAO_0000115>A dam. Constructed 1968.</obo:IAO_0000115>
        <oboInOwl:hasOBONamespace>GAZ</oboInOwl:hasOBONamespace>
        <oboInOwl:id>GAZ:00240243</oboInOwl:id>
        <rdfs:label>Lubisi Dam</rdfs:label>
    </owl:NamedIndividual>
    


    <!-- http://purl.obolibrary.org/obo/GAZ_00240244 -->

    <owl:NamedIndividual rdf:about="http://purl.obolibrary.org/obo/GAZ_00240244">
        <obo:RO_0001025 rdf:resource="http://purl.obolibrary.org/obo/GAZ_00239619"/>
        <oboInOwl:hasOBONamespace>GAZ</oboInOwl:hasOBONamespace>
        <oboInOwl:id>GAZ:00240244</oboInOwl:id>
        <rdfs:label>Emmarentia</rdfs:label>
    </owl:NamedIndividual>
    


    <!-- http://purl.obolibrary.org/obo/GAZ_00240245 -->

    <owl:NamedIndividual rdf:about="http://purl.obolibrary.org/obo/GAZ_00240245">
        <obo:RO_0001025 rdf:resource="http://purl.obolibrary.org/obo/GAZ_00239561"/>
        <obo:IAO_0000115>A dam. Constructed 1922.</obo:IAO_0000115>
        <oboInOwl:hasOBONamespace>GAZ</oboInOwl:hasOBONamespace>
        <oboInOwl:id>GAZ:00240245</oboInOwl:id>
        <rdfs:label>Darlington Dam</rdfs:label>
    </owl:NamedIndividual>
    


    <!-- http://purl.obolibrary.org/obo/GAZ_00240246 -->

    <owl:NamedIndividual rdf:about="http://purl.obolibrary.org/obo/GAZ_00240246">
        <obo:RO_0001025 rdf:resource="http://purl.obolibrary.org/obo/GAZ_00002819"/>
        <obo:IAO_0000115>A river.</obo:IAO_0000115>
        <oboInOwl:hasOBONamespace>GAZ</oboInOwl:hasOBONamespace>
        <oboInOwl:id>GAZ:00240246</oboInOwl:id>
        <rdfs:label>Krom River</rdfs:label>
    </owl:NamedIndividual>
    


    <!-- http://purl.obolibrary.org/obo/GAZ_00240247 -->

    <owl:NamedIndividual rdf:about="http://purl.obolibrary.org/obo/GAZ_00240247">
        <obo:RO_0001025 rdf:resource="http://purl.obolibrary.org/obo/GAZ_00002819"/>
        <obo:IAO_0000115>A river.</obo:IAO_0000115>
        <oboInOwl:hasOBONamespace>GAZ</oboInOwl:hasOBONamespace>
        <oboInOwl:id>GAZ:00240247</oboInOwl:id>
        <rdfs:label>Kromme River</rdfs:label>
    </owl:NamedIndividual>
    


    <!-- http://purl.obolibrary.org/obo/GAZ_00240248 -->

    <owl:NamedIndividual rdf:about="http://purl.obolibrary.org/obo/GAZ_00240248">
        <obo:RO_0001025 rdf:resource="http://purl.obolibrary.org/obo/GAZ_00239620"/>
        <obo:IAO_0000115>A location in South Africa. It is located about 10 miles west of Johannesburg.</obo:IAO_0000115>
        <oboInOwl:hasOBONamespace>GAZ</oboInOwl:hasOBONamespace>
        <oboInOwl:id>GAZ:00240248</oboInOwl:id>
        <rdfs:label>Florida</rdfs:label>
    </owl:NamedIndividual>
    


    <!-- http://purl.obolibrary.org/obo/GAZ_00240249 -->

    <owl:NamedIndividual rdf:about="http://purl.obolibrary.org/obo/GAZ_00240249">
        <obo:RO_0001025 rdf:resource="http://purl.obolibrary.org/obo/GAZ_00002819"/>
        <obo:IAO_0000115>A river.</obo:IAO_0000115>
        <oboInOwl:hasOBONamespace>GAZ</oboInOwl:hasOBONamespace>
        <oboInOwl:id>GAZ:00240249</oboInOwl:id>
        <rdfs:label>Mtata River</rdfs:label>
    </owl:NamedIndividual>
    


    <!-- http://purl.obolibrary.org/obo/GAZ_00240250 -->

    <owl:NamedIndividual rdf:about="http://purl.obolibrary.org/obo/GAZ_00240250">
        <obo:RO_0001025 rdf:resource="http://purl.obolibrary.org/obo/GAZ_00002819"/>
        <obo:IAO_0000115>A river.</obo:IAO_0000115>
        <oboInOwl:hasOBONamespace>GAZ</oboInOwl:hasOBONamespace>
        <oboInOwl:id>GAZ:00240250</oboInOwl:id>
        <rdfs:label>White Kei River</rdfs:label>
    </owl:NamedIndividual>
    


    <!-- http://purl.obolibrary.org/obo/GAZ_00240251 -->

    <owl:NamedIndividual rdf:about="http://purl.obolibrary.org/obo/GAZ_00240251">
        <obo:RO_0001025 rdf:resource="http://purl.obolibrary.org/obo/GAZ_00240246"/>
        <obo:IAO_0000115>A dam. Constructed 1982.</obo:IAO_0000115>
        <oboInOwl:hasOBONamespace>GAZ</oboInOwl:hasOBONamespace>
        <oboInOwl:id>GAZ:00240251</oboInOwl:id>
        <rdfs:label>Impofu Dam</rdfs:label>
    </owl:NamedIndividual>
    


    <!-- http://purl.obolibrary.org/obo/GAZ_00240252 -->

    <owl:NamedIndividual rdf:about="http://purl.obolibrary.org/obo/GAZ_00240252">
        <obo:RO_0001025 rdf:resource="http://purl.obolibrary.org/obo/GAZ_00240247"/>
        <obo:IAO_0000115>A dam. Constructed 1943.</obo:IAO_0000115>
        <oboInOwl:hasOBONamespace>GAZ</oboInOwl:hasOBONamespace>
        <oboInOwl:id>GAZ:00240252</oboInOwl:id>
        <rdfs:label>Churchill Dam</rdfs:label>
    </owl:NamedIndividual>
    


    <!-- http://purl.obolibrary.org/obo/GAZ_00240253 -->

    <owl:NamedIndividual rdf:about="http://purl.obolibrary.org/obo/GAZ_00240253">
        <obo:RO_0001025 rdf:resource="http://purl.obolibrary.org/obo/GAZ_00240249"/>
        <obo:IAO_0000115>A dam. Constructed 1977.</obo:IAO_0000115>
        <oboInOwl:hasOBONamespace>GAZ</oboInOwl:hasOBONamespace>
        <oboInOwl:id>GAZ:00240253</oboInOwl:id>
        <rdfs:label>Mthata Dam</rdfs:label>
    </owl:NamedIndividual>
    


    <!-- http://purl.obolibrary.org/obo/GAZ_00240254 -->

    <owl:NamedIndividual rdf:about="http://purl.obolibrary.org/obo/GAZ_00240254">
        <obo:RO_0001025 rdf:resource="http://purl.obolibrary.org/obo/GAZ_00240250"/>
        <obo:IAO_0000115>A dam. Constructed 1974.</obo:IAO_0000115>
        <oboInOwl:hasOBONamespace>GAZ</oboInOwl:hasOBONamespace>
        <oboInOwl:id>GAZ:00240254</oboInOwl:id>
        <rdfs:label>Xonxa Dam</rdfs:label>
    </owl:NamedIndividual>
    


    <!-- http://purl.obolibrary.org/obo/GAZ_00240255 -->

    <owl:NamedIndividual rdf:about="http://purl.obolibrary.org/obo/GAZ_00240255">
        <obo:RO_0001025 rdf:resource="http://purl.obolibrary.org/obo/GAZ_00002813"/>
        <obo:IAO_0000115>A river.</obo:IAO_0000115>
        <oboInOwl:hasOBONamespace>GAZ</oboInOwl:hasOBONamespace>
        <oboInOwl:id>GAZ:00240255</oboInOwl:id>
        <rdfs:label>Leeu River</rdfs:label>
    </owl:NamedIndividual>
    


    <!-- http://purl.obolibrary.org/obo/GAZ_00240256 -->

    <owl:NamedIndividual rdf:about="http://purl.obolibrary.org/obo/GAZ_00240256">
        <obo:RO_0001025 rdf:resource="http://purl.obolibrary.org/obo/GAZ_00240255"/>
        <obo:IAO_0000115>A dam. Constructed 1954.</obo:IAO_0000115>
        <oboInOwl:hasOBONamespace>GAZ</oboInOwl:hasOBONamespace>
        <oboInOwl:id>GAZ:00240256</oboInOwl:id>
        <rdfs:label>Armenia Dam</rdfs:label>
    </owl:NamedIndividual>
    


    <!-- http://purl.obolibrary.org/obo/GAZ_00240257 -->

    <owl:NamedIndividual rdf:about="http://purl.obolibrary.org/obo/GAZ_00240257">
        <obo:RO_0001025 rdf:resource="http://purl.obolibrary.org/obo/GAZ_00240192"/>
        <obo:IAO_0000115>A dam. Constructed 1960.</obo:IAO_0000115>
        <oboInOwl:hasOBONamespace>GAZ</oboInOwl:hasOBONamespace>
        <oboInOwl:id>GAZ:00240257</oboInOwl:id>
        <rdfs:label>Erfenis Dam</rdfs:label>
    </owl:NamedIndividual>
    


    <!-- http://purl.obolibrary.org/obo/GAZ_00240258 -->

    <owl:NamedIndividual rdf:about="http://purl.obolibrary.org/obo/GAZ_00240258">
        <obo:RO_0001025 rdf:resource="http://purl.obolibrary.org/obo/GAZ_00002813"/>
        <obo:IAO_0000115>A river.</obo:IAO_0000115>
        <oboInOwl:hasOBONamespace>GAZ</oboInOwl:hasOBONamespace>
        <oboInOwl:id>GAZ:00240258</oboInOwl:id>
        <rdfs:label>Wittespruit</rdfs:label>
    </owl:NamedIndividual>
    


    <!-- http://purl.obolibrary.org/obo/GAZ_00240259 -->

    <owl:NamedIndividual rdf:about="http://purl.obolibrary.org/obo/GAZ_00240259">
        <obo:RO_0001025 rdf:resource="http://purl.obolibrary.org/obo/GAZ_00240258"/>
        <obo:IAO_0000115>A dam. Constructed 1937.</obo:IAO_0000115>
        <oboInOwl:hasOBONamespace>GAZ</oboInOwl:hasOBONamespace>
        <oboInOwl:id>GAZ:00240259</oboInOwl:id>
        <rdfs:label>Egmont Dam</rdfs:label>
    </owl:NamedIndividual>
    


    <!-- http://purl.obolibrary.org/obo/GAZ_00240260 -->

    <owl:NamedIndividual rdf:about="http://purl.obolibrary.org/obo/GAZ_00240260">
        <obo:RO_0001025 rdf:resource="http://purl.obolibrary.org/obo/GAZ_00240190"/>
        <obo:IAO_0000115>A dam. Constructed 1960.</obo:IAO_0000115>
        <oboInOwl:hasOBONamespace>GAZ</oboInOwl:hasOBONamespace>
        <oboInOwl:id>GAZ:00240260</oboInOwl:id>
        <rdfs:label>Allemanskraal</rdfs:label>
    </owl:NamedIndividual>
    


    <!-- http://purl.obolibrary.org/obo/GAZ_00240261 -->

    <owl:NamedIndividual rdf:about="http://purl.obolibrary.org/obo/GAZ_00240261">
        <obo:IAO_0000115>A dam. Constructed 1938.</obo:IAO_0000115>
        <oboInOwl:hasOBONamespace>GAZ</oboInOwl:hasOBONamespace>
        <oboInOwl:id>GAZ:00240261</oboInOwl:id>
        <rdfs:label>Kalkfontein Dam</rdfs:label>
    </owl:NamedIndividual>
    


    <!-- http://purl.obolibrary.org/obo/GAZ_00240262 -->

    <owl:NamedIndividual rdf:about="http://purl.obolibrary.org/obo/GAZ_00240262">
        <obo:RO_0001025 rdf:resource="http://purl.obolibrary.org/obo/GAZ_00002813"/>
        <obo:IAO_0000115>A river.</obo:IAO_0000115>
        <oboInOwl:hasOBONamespace>GAZ</oboInOwl:hasOBONamespace>
        <oboInOwl:id>GAZ:00240262</oboInOwl:id>
        <rdfs:label>Rietspruit</rdfs:label>
    </owl:NamedIndividual>
    


    <!-- http://purl.obolibrary.org/obo/GAZ_00240263 -->

    <owl:NamedIndividual rdf:about="http://purl.obolibrary.org/obo/GAZ_00240263">
        <obo:RO_0001025 rdf:resource="http://purl.obolibrary.org/obo/GAZ_00240262"/>
        <obo:IAO_0000115>A dam. Constructed 1988.</obo:IAO_0000115>
        <oboInOwl:hasOBONamespace>GAZ</oboInOwl:hasOBONamespace>
        <oboInOwl:id>GAZ:00240263</oboInOwl:id>
        <rdfs:label>Knellpoort Dam</rdfs:label>
    </owl:NamedIndividual>
    


    <!-- http://purl.obolibrary.org/obo/GAZ_00240264 -->

    <owl:NamedIndividual rdf:about="http://purl.obolibrary.org/obo/GAZ_00240264">
        <obo:RO_0001025 rdf:resource="http://purl.obolibrary.org/obo/GAZ_00002812"/>
        <obo:IAO_0000115>A river.</obo:IAO_0000115>
        <oboInOwl:hasOBONamespace>GAZ</oboInOwl:hasOBONamespace>
        <oboInOwl:id>GAZ:00240264</oboInOwl:id>
        <rdfs:label>Klip River</rdfs:label>
    </owl:NamedIndividual>
    


    <!-- http://purl.obolibrary.org/obo/GAZ_00240265 -->

    <owl:NamedIndividual rdf:about="http://purl.obolibrary.org/obo/GAZ_00240265">
        <obo:RO_0001025 rdf:resource="http://purl.obolibrary.org/obo/GAZ_00002812"/>
        <obo:IAO_0000115>A river.</obo:IAO_0000115>
        <oboInOwl:hasOBONamespace>GAZ</oboInOwl:hasOBONamespace>
        <oboInOwl:id>GAZ:00240265</oboInOwl:id>
        <rdfs:label>Bivane River</rdfs:label>
    </owl:NamedIndividual>
    


    <!-- http://purl.obolibrary.org/obo/GAZ_00240266 -->

    <owl:NamedIndividual rdf:about="http://purl.obolibrary.org/obo/GAZ_00240266">
        <obo:RO_0001025 rdf:resource="http://purl.obolibrary.org/obo/GAZ_00002812"/>
        <obo:IAO_0000115>A river.</obo:IAO_0000115>
        <oboInOwl:hasOBONamespace>GAZ</oboInOwl:hasOBONamespace>
        <oboInOwl:id>GAZ:00240266</oboInOwl:id>
        <rdfs:label>Mhlatuze River</rdfs:label>
    </owl:NamedIndividual>
    


    <!-- http://purl.obolibrary.org/obo/GAZ_00240267 -->

    <owl:NamedIndividual rdf:about="http://purl.obolibrary.org/obo/GAZ_00240267">
        <obo:RO_0001025 rdf:resource="http://purl.obolibrary.org/obo/GAZ_00240265"/>
        <obo:IAO_0000115>A dam. Constructed 2000.</obo:IAO_0000115>
        <oboInOwl:hasOBONamespace>GAZ</oboInOwl:hasOBONamespace>
        <oboInOwl:id>GAZ:00240267</oboInOwl:id>
        <rdfs:label>Bivane Dam</rdfs:label>
    </owl:NamedIndividual>
    


    <!-- http://purl.obolibrary.org/obo/GAZ_00240268 -->

    <owl:NamedIndividual rdf:about="http://purl.obolibrary.org/obo/GAZ_00240268">
        <obo:RO_0001025 rdf:resource="http://purl.obolibrary.org/obo/GAZ_00240264"/>
        <obo:IAO_0000115>A dam. Constructed 1997.</obo:IAO_0000115>
        <oboInOwl:hasOBONamespace>GAZ</oboInOwl:hasOBONamespace>
        <oboInOwl:id>GAZ:00240268</oboInOwl:id>
        <rdfs:label>Qedusizi Dam</rdfs:label>
    </owl:NamedIndividual>
    


    <!-- http://purl.obolibrary.org/obo/GAZ_00240269 -->

    <owl:NamedIndividual rdf:about="http://purl.obolibrary.org/obo/GAZ_00240269">
        <obo:RO_0001025 rdf:resource="http://purl.obolibrary.org/obo/GAZ_00240266"/>
        <obo:IAO_0000115>A dam. Constructed 1982.</obo:IAO_0000115>
        <oboInOwl:hasOBONamespace>GAZ</oboInOwl:hasOBONamespace>
        <oboInOwl:id>GAZ:00240269</oboInOwl:id>
        <rdfs:label>Goedertrouw Dam</rdfs:label>
    </owl:NamedIndividual>
    


    <!-- http://purl.obolibrary.org/obo/GAZ_00240270 -->

    <owl:NamedIndividual rdf:about="http://purl.obolibrary.org/obo/GAZ_00240270">
        <obo:RO_0001025 rdf:resource="http://purl.obolibrary.org/obo/GAZ_00240264"/>
        <obo:IAO_0000115>A dam. Constructed 1950.</obo:IAO_0000115>
        <oboInOwl:hasOBONamespace>GAZ</oboInOwl:hasOBONamespace>
        <oboInOwl:id>GAZ:00240270</oboInOwl:id>
        <rdfs:label>Windsor Dam</rdfs:label>
    </owl:NamedIndividual>
    


    <!-- http://purl.obolibrary.org/obo/GAZ_00240271 -->

    <owl:NamedIndividual rdf:about="http://purl.obolibrary.org/obo/GAZ_00240271">
        <obo:RO_0001025 rdf:resource="http://purl.obolibrary.org/obo/GAZ_00002812"/>
        <obo:IAO_0000115>A river.</obo:IAO_0000115>
        <oboInOwl:hasOBONamespace>GAZ</oboInOwl:hasOBONamespace>
        <oboInOwl:id>GAZ:00240271</oboInOwl:id>
        <rdfs:label>Nsama River</rdfs:label>
    </owl:NamedIndividual>
    


    <!-- http://purl.obolibrary.org/obo/GAZ_00240272 -->

    <owl:NamedIndividual rdf:about="http://purl.obolibrary.org/obo/GAZ_00240272">
        <obo:RO_0001025 rdf:resource="http://purl.obolibrary.org/obo/GAZ_00240271"/>
        <obo:IAO_0000115>A dam. Constructed 1961.</obo:IAO_0000115>
        <oboInOwl:hasOBONamespace>GAZ</oboInOwl:hasOBONamespace>
        <oboInOwl:id>GAZ:00240272</oboInOwl:id>
        <rdfs:label>Ntshingwayo Dam</rdfs:label>
    </owl:NamedIndividual>
    


    <!-- http://purl.obolibrary.org/obo/GAZ_00240273 -->

    <owl:NamedIndividual rdf:about="http://purl.obolibrary.org/obo/GAZ_00240273">
        <obo:RO_0001025 rdf:resource="http://purl.obolibrary.org/obo/GAZ_00002814"/>
        <obo:IAO_0000115>A river.</obo:IAO_0000115>
        <oboInOwl:hasOBONamespace>GAZ</oboInOwl:hasOBONamespace>
        <oboInOwl:id>GAZ:00240273</oboInOwl:id>
        <rdfs:label>Middle Letaba River</rdfs:label>
    </owl:NamedIndividual>
    


    <!-- http://purl.obolibrary.org/obo/GAZ_00240274 -->

    <owl:NamedIndividual rdf:about="http://purl.obolibrary.org/obo/GAZ_00240274">
        <obo:RO_0001025 rdf:resource="http://purl.obolibrary.org/obo/GAZ_00240273"/>
        <obo:IAO_0000115>A dam. Constructed 1984.</obo:IAO_0000115>
        <oboInOwl:hasOBONamespace>GAZ</oboInOwl:hasOBONamespace>
        <oboInOwl:id>GAZ:00240274</oboInOwl:id>
        <rdfs:label>Middle Letaba Dam</rdfs:label>
    </owl:NamedIndividual>
    


    <!-- http://purl.obolibrary.org/obo/GAZ_00240275 -->

    <owl:NamedIndividual rdf:about="http://purl.obolibrary.org/obo/GAZ_00240275">
        <obo:RO_0001025 rdf:resource="http://purl.obolibrary.org/obo/GAZ_00240203"/>
        <obo:IAO_0000115>A dam. Constructed 1980.</obo:IAO_0000115>
        <oboInOwl:hasOBONamespace>GAZ</oboInOwl:hasOBONamespace>
        <oboInOwl:id>GAZ:00240275</oboInOwl:id>
        <rdfs:label>Mokolo Dam</rdfs:label>
    </owl:NamedIndividual>
    


    <!-- http://purl.obolibrary.org/obo/GAZ_00240276 -->

    <owl:NamedIndividual rdf:about="http://purl.obolibrary.org/obo/GAZ_00240276">
        <obo:RO_0001025 rdf:resource="http://purl.obolibrary.org/obo/GAZ_00002814"/>
        <obo:IAO_0000115>A river.</obo:IAO_0000115>
        <oboInOwl:hasOBONamespace>GAZ</oboInOwl:hasOBONamespace>
        <oboInOwl:id>GAZ:00240276</oboInOwl:id>
        <rdfs:label>Mutshindudi River</rdfs:label>
    </owl:NamedIndividual>
    


    <!-- http://purl.obolibrary.org/obo/GAZ_00240277 -->

    <owl:NamedIndividual rdf:about="http://purl.obolibrary.org/obo/GAZ_00240277">
        <obo:RO_0001025 rdf:resource="http://purl.obolibrary.org/obo/GAZ_00240276"/>
        <obo:IAO_0000115>A dam. Constructed 1971.</obo:IAO_0000115>
        <oboInOwl:hasOBONamespace>GAZ</oboInOwl:hasOBONamespace>
        <oboInOwl:id>GAZ:00240277</oboInOwl:id>
        <rdfs:label>Phiphidi Dam</rdfs:label>
    </owl:NamedIndividual>
    


    <!-- http://purl.obolibrary.org/obo/GAZ_00240447 -->

    <owl:NamedIndividual rdf:about="http://purl.obolibrary.org/obo/GAZ_00240447">
        <obo:RO_0001025 rdf:resource="http://purl.obolibrary.org/obo/GAZ_00240244"/>
        <obo:IAO_0000115>A reservoir.</obo:IAO_0000115>
        <oboInOwl:hasOBONamespace>GAZ</oboInOwl:hasOBONamespace>
        <oboInOwl:id>GAZ:00240447</oboInOwl:id>
        <rdfs:label>Emmarentia Dam</rdfs:label>
    </owl:NamedIndividual>
    


    <!-- http://purl.obolibrary.org/obo/GAZ_00246864 -->

    <owl:NamedIndividual rdf:about="http://purl.obolibrary.org/obo/GAZ_00246864">
        <rdf:type rdf:resource="http://purl.obolibrary.org/obo/ENVO_00000309"/>
        <obo:RO_0001025 rdf:resource="http://purl.obolibrary.org/obo/GAZ_00076291"/>
        <obo:IAO_0000115>A pan.</obo:IAO_0000115>
        <oboInOwl:hasOBONamespace>GAZ</oboInOwl:hasOBONamespace>
        <oboInOwl:id>GAZ:00246864</oboInOwl:id>
        <rdfs:label>Kgama Kgama Pan</rdfs:label>
    </owl:NamedIndividual>
    


    <!-- http://purl.obolibrary.org/obo/GAZ_00246865 -->

    <owl:NamedIndividual rdf:about="http://purl.obolibrary.org/obo/GAZ_00246865">
        <obo:IAO_0000115>A reservoir impounded by the Shashe Dam.</obo:IAO_0000115>
        <oboInOwl:hasOBONamespace>GAZ</oboInOwl:hasOBONamespace>
        <oboInOwl:id>GAZ:00246865</oboInOwl:id>
        <rdfs:label>Shashe Impoundment</rdfs:label>
    </owl:NamedIndividual>
    


    <!-- http://purl.obolibrary.org/obo/GAZ_00252370 -->

    <owl:NamedIndividual rdf:about="http://purl.obolibrary.org/obo/GAZ_00252370">
        <obo:IAO_0000115>A dam.</obo:IAO_0000115>
        <oboInOwl:hasOBONamespace>GAZ</oboInOwl:hasOBONamespace>
        <oboInOwl:id>GAZ:00252370</oboInOwl:id>
        <rdfs:label>Barragem de Macarretane</rdfs:label>
    </owl:NamedIndividual>
    


    <!-- http://purl.obolibrary.org/obo/GAZ_00252372 -->

    <owl:NamedIndividual rdf:about="http://purl.obolibrary.org/obo/GAZ_00252372">
        <obo:IAO_0000115>A dam.</obo:IAO_0000115>
        <oboInOwl:hasOBONamespace>GAZ</oboInOwl:hasOBONamespace>
        <oboInOwl:id>GAZ:00252372</oboInOwl:id>
        <rdfs:label>Renosterkop Dam</rdfs:label>
    </owl:NamedIndividual>
    


    <!-- http://purl.obolibrary.org/obo/GAZ_00252375 -->

    <owl:NamedIndividual rdf:about="http://purl.obolibrary.org/obo/GAZ_00252375">
        <obo:IAO_0000115>A river.</obo:IAO_0000115>
        <oboInOwl:hasOBONamespace>GAZ</oboInOwl:hasOBONamespace>
        <oboInOwl:id>GAZ:00252375</oboInOwl:id>
        <rdfs:label>Rust de Winter Dam</rdfs:label>
    </owl:NamedIndividual>
    


    <!-- http://purl.obolibrary.org/obo/GAZ_00252376 -->

    <owl:NamedIndividual rdf:about="http://purl.obolibrary.org/obo/GAZ_00252376">
        <obo:IAO_0000115>A dam.</obo:IAO_0000115>
        <oboInOwl:hasOBONamespace>GAZ</oboInOwl:hasOBONamespace>
        <oboInOwl:id>GAZ:00252376</oboInOwl:id>
        <rdfs:label>Blyderivierspoort Dam</rdfs:label>
    </owl:NamedIndividual>
    


    <!-- http://purl.obolibrary.org/obo/GAZ_00252377 -->

    <owl:NamedIndividual rdf:about="http://purl.obolibrary.org/obo/GAZ_00252377">
        <obo:IAO_0000115>A reservoir. Impounded by Middelburg Dam. Constructed 1978.</obo:IAO_0000115>
        <oboInOwl:hasOBONamespace>GAZ</oboInOwl:hasOBONamespace>
        <oboInOwl:id>GAZ:00252377</oboInOwl:id>
        <rdfs:label>Middelburg Dam Reservoir</rdfs:label>
    </owl:NamedIndividual>
    


    <!-- http://purl.obolibrary.org/obo/GAZ_00252378 -->

    <owl:NamedIndividual rdf:about="http://purl.obolibrary.org/obo/GAZ_00252378">
        <obo:IAO_0000115>A dam on the Klein Olifants River, near Middelburg, Mpumalanga, South Africa. Impounds Middelburg Dam Reservoir. Constructed 1978.</obo:IAO_0000115>
        <oboInOwl:hasOBONamespace>GAZ</oboInOwl:hasOBONamespace>
        <oboInOwl:id>GAZ:00252378</oboInOwl:id>
        <rdfs:label>Middelburg Dam</rdfs:label>
    </owl:NamedIndividual>
    


    <!-- http://purl.obolibrary.org/obo/GAZ_00252379 -->

    <owl:NamedIndividual rdf:about="http://purl.obolibrary.org/obo/GAZ_00252379">
        <obo:IAO_0000115>A river. It arises from several streams which have their origins on the borders of the Gonarhezou Game Reserve in SE Zimbabwe and in the swamps on the southern boundary of the Zinhave National Park. They form a great dendritic system anastomosing at a point at the NE tip of the Banhine National Park. From here the Changane flows nearly due south, between two low plateau blocks, receiving more tributaries on its west bank.</obo:IAO_0000115>
        <oboInOwl:hasOBONamespace>GAZ</oboInOwl:hasOBONamespace>
        <oboInOwl:id>GAZ:00252379</oboInOwl:id>
        <rdfs:label>Rio Changane</rdfs:label>
    </owl:NamedIndividual>
    


    <!-- http://purl.obolibrary.org/obo/GAZ_00252380 -->

    <owl:NamedIndividual rdf:about="http://purl.obolibrary.org/obo/GAZ_00252380">
        <obo:IAO_0000115>A reservoir. Impounded by the Arabie Dam.</obo:IAO_0000115>
        <oboInOwl:hasOBONamespace>GAZ</oboInOwl:hasOBONamespace>
        <oboInOwl:id>GAZ:00252380</oboInOwl:id>
        <rdfs:label>Arabie Dam Reservoir</rdfs:label>
    </owl:NamedIndividual>
    


    <!-- http://purl.obolibrary.org/obo/GAZ_00252381 -->

    <owl:NamedIndividual rdf:about="http://purl.obolibrary.org/obo/GAZ_00252381">
        <oboInOwl:hasOBONamespace>GAZ</oboInOwl:hasOBONamespace>
        <oboInOwl:id>GAZ:00252381</oboInOwl:id>
        <rdfs:label>Phalaborwa Barrage</rdfs:label>
    </owl:NamedIndividual>
    


    <!-- http://purl.obolibrary.org/obo/GAZ_00252425 -->

    <owl:NamedIndividual rdf:about="http://purl.obolibrary.org/obo/GAZ_00252425">
        <obo:RO_0001025 rdf:resource="http://purl.obolibrary.org/obo/GAZ_00239490"/>
        <obo:IAO_0000115>A reservoir. Impounded by Naute Dam.</obo:IAO_0000115>
        <oboInOwl:hasOBONamespace>GAZ</oboInOwl:hasOBONamespace>
        <oboInOwl:id>GAZ:00252425</oboInOwl:id>
        <rdfs:label>Naute Reservoir</rdfs:label>
    </owl:NamedIndividual>
    


    <!-- http://purl.obolibrary.org/obo/GAZ_00255961 -->

    <owl:NamedIndividual rdf:about="http://purl.obolibrary.org/obo/GAZ_00255961">
        <obo:RO_0001025 rdf:resource="http://purl.obolibrary.org/obo/GAZ_00146602"/>
        <obo:IAO_0000115>An island.</obo:IAO_0000115>
        <oboInOwl:hasOBONamespace>GAZ</oboInOwl:hasOBONamespace>
        <oboInOwl:id>GAZ:00255961</oboInOwl:id>
        <rdfs:label>Meeuw Island</rdfs:label>
    </owl:NamedIndividual>
    


    <!-- http://purl.obolibrary.org/obo/GAZ_00255962 -->

    <owl:NamedIndividual rdf:about="http://purl.obolibrary.org/obo/GAZ_00255962">
        <obo:RO_0001025 rdf:resource="http://purl.obolibrary.org/obo/GAZ_00146602"/>
        <obo:IAO_0000115>An island.</obo:IAO_0000115>
        <oboInOwl:hasOBONamespace>GAZ</oboInOwl:hasOBONamespace>
        <oboInOwl:id>GAZ:00255962</oboInOwl:id>
        <rdfs:label>Schaapen Island</rdfs:label>
    </owl:NamedIndividual>
    


    <!-- http://purl.obolibrary.org/obo/GAZ_00255963 -->

    <owl:NamedIndividual rdf:about="http://purl.obolibrary.org/obo/GAZ_00255963">
        <obo:RO_0001025 rdf:resource="http://purl.obolibrary.org/obo/GAZ_00002819"/>
        <obo:IAO_0000115>A river.</obo:IAO_0000115>
        <oboInOwl:hasOBONamespace>GAZ</oboInOwl:hasOBONamespace>
        <oboInOwl:id>GAZ:00255963</oboInOwl:id>
        <rdfs:label>Mngazana River</rdfs:label>
    </owl:NamedIndividual>
    


    <!-- http://purl.obolibrary.org/obo/GAZ_00255964 -->

    <owl:NamedIndividual rdf:about="http://purl.obolibrary.org/obo/GAZ_00255964">
        <obo:RO_0001025 rdf:resource="http://purl.obolibrary.org/obo/GAZ_00002812"/>
        <obo:IAO_0000115>A wetland.</obo:IAO_0000115>
        <oboInOwl:hasOBONamespace>GAZ</oboInOwl:hasOBONamespace>
        <oboInOwl:id>GAZ:00255964</oboInOwl:id>
        <rdfs:label>South Mosi Swamp</rdfs:label>
    </owl:NamedIndividual>
    


    <!-- http://purl.obolibrary.org/obo/GAZ_00255965 -->

    <owl:NamedIndividual rdf:about="http://purl.obolibrary.org/obo/GAZ_00255965">
        <obo:RO_0001025 rdf:resource="http://purl.obolibrary.org/obo/GAZ_00255964"/>
        <obo:IAO_0000115>A lake.</obo:IAO_0000115>
        <oboInOwl:hasOBONamespace>GAZ</oboInOwl:hasOBONamespace>
        <oboInOwl:id>GAZ:00255965</oboInOwl:id>
        <rdfs:label>Ndlaka</rdfs:label>
    </owl:NamedIndividual>
    


    <!-- http://purl.obolibrary.org/obo/GAZ_00255966 -->

    <owl:NamedIndividual rdf:about="http://purl.obolibrary.org/obo/GAZ_00255966">
        <obo:RO_0001025 rdf:resource="http://purl.obolibrary.org/obo/GAZ_00255964"/>
        <obo:IAO_0000115>A lake.</obo:IAO_0000115>
        <oboInOwl:hasOBONamespace>GAZ</oboInOwl:hasOBONamespace>
        <oboInOwl:id>GAZ:00255966</oboInOwl:id>
        <rdfs:label>Demezane</rdfs:label>
    </owl:NamedIndividual>
    


    <!-- http://purl.obolibrary.org/obo/GAZ_00255967 -->

    <owl:NamedIndividual rdf:about="http://purl.obolibrary.org/obo/GAZ_00255967">
        <obo:RO_0001025 rdf:resource="http://purl.obolibrary.org/obo/GAZ_00255964"/>
        <obo:IAO_0000115>A lake.</obo:IAO_0000115>
        <oboInOwl:hasOBONamespace>GAZ</oboInOwl:hasOBONamespace>
        <oboInOwl:id>GAZ:00255967</oboInOwl:id>
        <rdfs:label>Mbazwan</rdfs:label>
    </owl:NamedIndividual>
    


    <!-- http://purl.obolibrary.org/obo/GAZ_00255968 -->

    <owl:NamedIndividual rdf:about="http://purl.obolibrary.org/obo/GAZ_00255968">
        <obo:RO_0001025 rdf:resource="http://purl.obolibrary.org/obo/GAZ_00255964"/>
        <obo:IAO_0000115>A lake.</obo:IAO_0000115>
        <oboInOwl:hasOBONamespace>GAZ</oboInOwl:hasOBONamespace>
        <oboInOwl:id>GAZ:00255968</oboInOwl:id>
        <rdfs:label>Butterfly</rdfs:label>
    </owl:NamedIndividual>
    


    <!-- http://purl.obolibrary.org/obo/GAZ_00255969 -->

    <owl:NamedIndividual rdf:about="http://purl.obolibrary.org/obo/GAZ_00255969">
        <obo:RO_0001025 rdf:resource="http://purl.obolibrary.org/obo/GAZ_00255964"/>
        <obo:IAO_0000115>A delta where the Mkuze River enters Mosi Swamp.</obo:IAO_0000115>
        <oboInOwl:hasOBONamespace>GAZ</oboInOwl:hasOBONamespace>
        <oboInOwl:id>GAZ:00255969</oboInOwl:id>
        <rdfs:label>Mkuze River Delta</rdfs:label>
    </owl:NamedIndividual>
    


    <!-- http://purl.obolibrary.org/obo/GAZ_00255970 -->

    <owl:NamedIndividual rdf:about="http://purl.obolibrary.org/obo/GAZ_00255970">
        <obo:RO_0001025 rdf:resource="http://purl.obolibrary.org/obo/GAZ_00255969"/>
        <obo:IAO_0000115>A lake.</obo:IAO_0000115>
        <oboInOwl:hasOBONamespace>GAZ</oboInOwl:hasOBONamespace>
        <oboInOwl:id>GAZ:00255970</oboInOwl:id>
        <rdfs:label>Mpempe Lake</rdfs:label>
    </owl:NamedIndividual>
    


    <!-- http://purl.obolibrary.org/obo/GAZ_00255971 -->

    <owl:NamedIndividual rdf:about="http://purl.obolibrary.org/obo/GAZ_00255971">
        <obo:RO_0001025 rdf:resource="http://purl.obolibrary.org/obo/GAZ_00255969"/>
        <obo:IAO_0000115>A lake.</obo:IAO_0000115>
        <oboInOwl:hasOBONamespace>GAZ</oboInOwl:hasOBONamespace>
        <oboInOwl:id>GAZ:00255971</oboInOwl:id>
        <rdfs:label>Ntshangwe Lake</rdfs:label>
    </owl:NamedIndividual>
    


    <!-- http://purl.obolibrary.org/obo/GAZ_00255972 -->

    <owl:NamedIndividual rdf:about="http://purl.obolibrary.org/obo/GAZ_00255972">
        <obo:RO_0001025 rdf:resource="http://purl.obolibrary.org/obo/GAZ_00255969"/>
        <obo:IAO_0000115>A lake.</obo:IAO_0000115>
        <oboInOwl:hasOBONamespace>GAZ</oboInOwl:hasOBONamespace>
        <oboInOwl:id>GAZ:00255972</oboInOwl:id>
        <rdfs:label>Mdlanzi Lake</rdfs:label>
    </owl:NamedIndividual>
    


    <!-- http://purl.obolibrary.org/obo/GAZ_00255973 -->

    <owl:NamedIndividual rdf:about="http://purl.obolibrary.org/obo/GAZ_00255973">
        <obo:RO_0001025 rdf:resource="http://purl.obolibrary.org/obo/GAZ_00255969"/>
        <obo:IAO_0000115>A lake.</obo:IAO_0000115>
        <oboInOwl:hasOBONamespace>GAZ</oboInOwl:hasOBONamespace>
        <oboInOwl:id>GAZ:00255973</oboInOwl:id>
        <rdfs:label>Tshanetsha Lake</rdfs:label>
    </owl:NamedIndividual>
    


    <!-- http://purl.obolibrary.org/obo/GAZ_00255975 -->

    <owl:NamedIndividual rdf:about="http://purl.obolibrary.org/obo/GAZ_00255975">
        <obo:RO_0001025 rdf:resource="http://purl.obolibrary.org/obo/GAZ_00002816"/>
        <obo:IAO_0000115>An endorheic lake. It is semi-permanent but may dry almost completely once in every 10 years.</obo:IAO_0000115>
        <oboInOwl:hasOBONamespace>GAZ</oboInOwl:hasOBONamespace>
        <oboInOwl:id>GAZ:00255975</oboInOwl:id>
        <rdfs:label>Lake Chrissie</rdfs:label>
    </owl:NamedIndividual>
    


    <!-- http://purl.obolibrary.org/obo/GAZ_00255976 -->

    <owl:NamedIndividual rdf:about="http://purl.obolibrary.org/obo/GAZ_00255976">
        <obo:RO_0001025 rdf:resource="http://purl.obolibrary.org/obo/GAZ_00002816"/>
        <obo:IAO_0000115>A lake/pan.</obo:IAO_0000115>
        <oboInOwl:hasOBONamespace>GAZ</oboInOwl:hasOBONamespace>
        <oboInOwl:id>GAZ:00255976</oboInOwl:id>
        <rdfs:label>Lake Banagher</rdfs:label>
    </owl:NamedIndividual>
    


    <!-- http://purl.obolibrary.org/obo/GAZ_00255977 -->

    <owl:NamedIndividual rdf:about="http://purl.obolibrary.org/obo/GAZ_00255977">
        <obo:RO_0001025 rdf:resource="http://purl.obolibrary.org/obo/GAZ_00002811"/>
        <obo:IAO_0000115>A lake/pan. Located N opf Barberspan.</obo:IAO_0000115>
        <oboInOwl:hasOBONamespace>GAZ</oboInOwl:hasOBONamespace>
        <oboInOwl:id>GAZ:00255977</oboInOwl:id>
        <rdfs:label>Leeupan</rdfs:label>
    </owl:NamedIndividual>
    


    <!-- http://purl.obolibrary.org/obo/GAZ_00260982 -->

    <owl:NamedIndividual rdf:about="http://purl.obolibrary.org/obo/GAZ_00260982">
        <obo:RO_0001025 rdf:resource="http://purl.obolibrary.org/obo/GAZ_00075392"/>
        <obo:RO_0001025 rdf:resource="http://purl.obolibrary.org/obo/GAZ_00237606"/>
        <obo:IAO_0000115>Lakes. A cluster of large perennial pools in the bed of the Runde River.</obo:IAO_0000115>
        <oboInOwl:hasOBONamespace>GAZ</oboInOwl:hasOBONamespace>
        <oboInOwl:id>GAZ:00260982</oboInOwl:id>
        <rdfs:label>Chipinda Pools</rdfs:label>
    </owl:NamedIndividual>
    


    <!-- http://purl.obolibrary.org/obo/GAZ_00260984 -->

    <owl:NamedIndividual rdf:about="http://purl.obolibrary.org/obo/GAZ_00260984">
        <rdf:type rdf:resource="http://purl.obolibrary.org/obo/ENVO_00000309"/>
        <obo:RO_0001025 rdf:resource="http://purl.obolibrary.org/obo/GAZ_00075394"/>
        <obo:IAO_0000115>A pan on a stretch of floodplain of the Mwenezi River.</obo:IAO_0000115>
        <oboInOwl:hasOBONamespace>GAZ</oboInOwl:hasOBONamespace>
        <oboInOwl:id>GAZ:00260984</oboInOwl:id>
        <rdfs:label>Manjinji Pan</rdfs:label>
    </owl:NamedIndividual>
    


    <!-- http://purl.obolibrary.org/obo/GAZ_00260985 -->

    <owl:NamedIndividual rdf:about="http://purl.obolibrary.org/obo/GAZ_00260985">
        <obo:RO_0001025 rdf:resource="http://purl.obolibrary.org/obo/GAZ_00075392"/>
        <obo:IAO_0000115>A series of shllow pans.</obo:IAO_0000115>
        <oboInOwl:hasOBONamespace>GAZ</oboInOwl:hasOBONamespace>
        <oboInOwl:id>GAZ:00260985</oboInOwl:id>
        <rdfs:label>Gorhwe Pans</rdfs:label>
    </owl:NamedIndividual>
    


    <!-- http://purl.obolibrary.org/obo/GAZ_00261007 -->

    <owl:NamedIndividual rdf:about="http://purl.obolibrary.org/obo/GAZ_00261007">
        <obo:RO_0001025 rdf:resource="http://purl.obolibrary.org/obo/GAZ_00237631"/>
        <obo:IAO_0000115>A reservoir. Impounded by Kyle Dam.</obo:IAO_0000115>
        <oboInOwl:hasOBONamespace>GAZ</oboInOwl:hasOBONamespace>
        <oboInOwl:id>GAZ:00261007</oboInOwl:id>
        <rdfs:label>Lake Kyle</rdfs:label>
    </owl:NamedIndividual>
    


    <!-- http://purl.obolibrary.org/obo/GAZ_00261014 -->

    <owl:NamedIndividual rdf:about="http://purl.obolibrary.org/obo/GAZ_00261014">
        <obo:IAO_0000115>A reservoir.</obo:IAO_0000115>
        <oboInOwl:hasOBONamespace>GAZ</oboInOwl:hasOBONamespace>
        <oboInOwl:id>GAZ:00261014</oboInOwl:id>
        <rdfs:label>Lake MacDougall</rdfs:label>
    </owl:NamedIndividual>
    


    <!-- http://purl.obolibrary.org/obo/GAZ_00281455 -->

    <owl:NamedIndividual rdf:about="http://purl.obolibrary.org/obo/GAZ_00281455">
        <obo:RO_0001025 rdf:resource="http://purl.obolibrary.org/obo/GAZ_00002816"/>
    </owl:NamedIndividual>
    


    <!-- http://purl.obolibrary.org/obo/GAZ_00281457 -->

    <owl:NamedIndividual rdf:about="http://purl.obolibrary.org/obo/GAZ_00281457">
        <obo:RO_0001025 rdf:resource="http://purl.obolibrary.org/obo/GAZ_00002817"/>
        <obo:IAO_0000115>A cave in a limestone cliff on the Southern Cape coast in South Africa. It is an archaeological site.</obo:IAO_0000115>
        <oboInOwl:hasOBONamespace>GAZ</oboInOwl:hasOBONamespace>
        <oboInOwl:id>GAZ:00281457</oboInOwl:id>
        <rdfs:label>Blombos Cave</rdfs:label>
    </owl:NamedIndividual>
    


    <!-- http://purl.obolibrary.org/obo/GAZ_00281458 -->

    <owl:NamedIndividual rdf:about="http://purl.obolibrary.org/obo/GAZ_00281458">
        <obo:IAO_0000115>An archeological site. A rock shelter on the western scarp of the Lebombo Mountains in KwaZulu-Natal near the border between South Africa and Swaziland.</obo:IAO_0000115>
        <oboInOwl:hasOBONamespace>GAZ</oboInOwl:hasOBONamespace>
        <oboInOwl:id>GAZ:00281458</oboInOwl:id>
        <rdfs:label>Border Cave</rdfs:label>
    </owl:NamedIndividual>
    


    <!-- http://purl.obolibrary.org/obo/GAZ_00281459 -->

    <owl:NamedIndividual rdf:about="http://purl.obolibrary.org/obo/GAZ_00281459">
        <obo:RO_0001025 rdf:resource="http://purl.obolibrary.org/obo/GAZ_00076120"/>
        <obo:IAO_0000115>Caves located in Precambrian limestones at the foothills of the Swartberg range near the town of Oudtshoorn in the Western Cape Province of South Africa.</obo:IAO_0000115>
        <oboInOwl:hasOBONamespace>GAZ</oboInOwl:hasOBONamespace>
        <oboInOwl:id>GAZ:00281459</oboInOwl:id>
        <rdfs:label>Cango Caves</rdfs:label>
    </owl:NamedIndividual>
    


    <!-- http://purl.obolibrary.org/obo/GAZ_00281460 -->

    <owl:NamedIndividual rdf:about="http://purl.obolibrary.org/obo/GAZ_00281460">
        <obo:RO_0001025 rdf:resource="http://purl.obolibrary.org/obo/GAZ_00032870"/>
        <obo:IAO_0000115>An archeological site. A rich Early Stone Age situated outside Barkly West in the Northern Cape, South Africa.</obo:IAO_0000115>
        <oboInOwl:hasOBONamespace>GAZ</oboInOwl:hasOBONamespace>
        <oboInOwl:id>GAZ:00281460</oboInOwl:id>
        <rdfs:label>Canteen Kopje</rdfs:label>
    </owl:NamedIndividual>
    


    <!-- http://purl.obolibrary.org/obo/GAZ_00281461 -->

    <owl:NamedIndividual rdf:about="http://purl.obolibrary.org/obo/GAZ_00281461">
        <obo:RO_0001025 rdf:resource="http://purl.obolibrary.org/obo/GAZ_00032856"/>
        <obo:IAO_0000115>An archeological site. A rock cave in Western Cape, South Africa in which has been found some of the earliest evidence of the human use of symbols.</obo:IAO_0000115>
        <oboInOwl:hasOBONamespace>GAZ</oboInOwl:hasOBONamespace>
        <oboInOwl:id>GAZ:00281461</oboInOwl:id>
        <rdfs:label>Diepkloof Rock Shelter</rdfs:label>
    </owl:NamedIndividual>
    


    <!-- http://purl.obolibrary.org/obo/GAZ_00281462 -->

    <owl:NamedIndividual rdf:about="http://purl.obolibrary.org/obo/GAZ_00281462">
        <obo:RO_0001025 rdf:resource="http://purl.obolibrary.org/obo/GAZ_00002818"/>
        <obo:IAO_0000115>An archeological site. A rock engraving or petroglyph site in the bed of the Riet River close to the town of Plooysburg, near Kimberley, Northern Cape, South Africa.</obo:IAO_0000115>
        <oboInOwl:hasOBONamespace>GAZ</oboInOwl:hasOBONamespace>
        <oboInOwl:id>GAZ:00281462</oboInOwl:id>
        <rdfs:label>Driekops Eiland</rdfs:label>
    </owl:NamedIndividual>
    


    <!-- http://purl.obolibrary.org/obo/GAZ_00281463 -->

    <owl:NamedIndividual rdf:about="http://purl.obolibrary.org/obo/GAZ_00281463">
        <obo:RO_0001025 rdf:resource="http://purl.obolibrary.org/obo/GAZ_00002817"/>
        <obo:IAO_0000115>Archaeological sites near Cape Town in South Africa.</obo:IAO_0000115>
        <oboInOwl:hasOBONamespace>GAZ</oboInOwl:hasOBONamespace>
        <oboInOwl:id>GAZ:00281463</oboInOwl:id>
        <rdfs:label>Duinefontein</rdfs:label>
    </owl:NamedIndividual>
    


    <!-- http://purl.obolibrary.org/obo/GAZ_00281464 -->

    <owl:NamedIndividual rdf:about="http://purl.obolibrary.org/obo/GAZ_00281464">
        <obo:RO_0001025 rdf:resource="http://purl.obolibrary.org/obo/GAZ_00076025"/>
        <obo:IAO_0000115>An archaeological site in Makhado municipality, Vhembe district, in the north of South Africa.</obo:IAO_0000115>
        <oboInOwl:hasOBONamespace>GAZ</oboInOwl:hasOBONamespace>
        <oboInOwl:id>GAZ:00281464</oboInOwl:id>
        <rdfs:label>Dzata Ruins</rdfs:label>
    </owl:NamedIndividual>
    


    <!-- http://purl.obolibrary.org/obo/GAZ_00281465 -->

    <owl:NamedIndividual rdf:about="http://purl.obolibrary.org/obo/GAZ_00281465">
        <obo:RO_0001025 rdf:resource="http://purl.obolibrary.org/obo/GAZ_00002813"/>
        <obo:IAO_0000115>A populated place.</obo:IAO_0000115>
        <oboInOwl:hasOBONamespace>GAZ</oboInOwl:hasOBONamespace>
        <oboInOwl:id>GAZ:00281465</oboInOwl:id>
        <rdfs:label>Brandfort</rdfs:label>
    </owl:NamedIndividual>
    


    <!-- http://purl.obolibrary.org/obo/GAZ_00281466 -->

    <owl:NamedIndividual rdf:about="http://purl.obolibrary.org/obo/GAZ_00281466">
        <obo:RO_0001025 rdf:resource="http://purl.obolibrary.org/obo/GAZ_00281465"/>
        <obo:IAO_0000115>An archaeological and paleontological site.</obo:IAO_0000115>
        <oboInOwl:hasOBONamespace>GAZ</oboInOwl:hasOBONamespace>
        <oboInOwl:id>GAZ:00281466</oboInOwl:id>
        <rdfs:label>Florisbad fossil site</rdfs:label>
    </owl:NamedIndividual>
    


    <!-- http://purl.obolibrary.org/obo/GAZ_00281467 -->

    <owl:NamedIndividual rdf:about="http://purl.obolibrary.org/obo/GAZ_00281467">
        <rdf:type rdf:resource="http://purl.obolibrary.org/obo/ENVO_00000106"/>
        <obo:RO_0001025 rdf:resource="http://purl.obolibrary.org/obo/GAZ_00002818"/>
        <obo:IAO_0000115>A range of hills in the Northern Cape province of South Africa, stretching SSW from Kuruman, where the range is known as the Kuruman Hills, to Prieska.</obo:IAO_0000115>
        <oboInOwl:hasOBONamespace>GAZ</oboInOwl:hasOBONamespace>
        <oboInOwl:id>GAZ:00281467</oboInOwl:id>
        <rdfs:label>Asbestos Mountains</rdfs:label>
    </owl:NamedIndividual>
    


    <!-- http://purl.obolibrary.org/obo/GAZ_00281468 -->

    <owl:NamedIndividual rdf:about="http://purl.obolibrary.org/obo/GAZ_00281468">
        <obo:RO_0001025 rdf:resource="http://purl.obolibrary.org/obo/GAZ_00281467"/>
        <obo:IAO_0000115>An archaeological site, formed originally as an ancient solution cavity in Dolomite rocks of the Kuruman Hills, situated between Danielskuil and Kuruman in the Northern Cape Province, South Africa.</obo:IAO_0000115>
        <oboInOwl:hasOBONamespace>GAZ</oboInOwl:hasOBONamespace>
        <oboInOwl:id>GAZ:00281468</oboInOwl:id>
        <rdfs:label>Wonderwerk Cave</rdfs:label>
    </owl:NamedIndividual>
    


    <!-- http://purl.obolibrary.org/obo/GAZ_00281469 -->

    <owl:NamedIndividual rdf:about="http://purl.obolibrary.org/obo/GAZ_00281469">
        <obo:RO_0001025 rdf:resource="http://purl.obolibrary.org/obo/GAZ_00002818"/>
        <obo:IAO_0000115>An archeological site. A rock engraving site with visitor centre on land owned by the !Xun and Khwe San situated about 16 km from Kimberley, Northern Cape, South Africa.</obo:IAO_0000115>
        <oboInOwl:hasOBONamespace>GAZ</oboInOwl:hasOBONamespace>
        <oboInOwl:id>GAZ:00281469</oboInOwl:id>
        <rdfs:label>Wildebeest Kuil Rock Art Centre</rdfs:label>
    </owl:NamedIndividual>
    


    <!-- http://purl.obolibrary.org/obo/GAZ_00281470 -->

    <owl:NamedIndividual rdf:about="http://purl.obolibrary.org/obo/GAZ_00281470">
        <obo:RO_0001025 rdf:resource="http://purl.obolibrary.org/obo/GAZ_00002811"/>
        <obo:IAO_0000115>A populated place.</obo:IAO_0000115>
        <oboInOwl:hasOBONamespace>GAZ</oboInOwl:hasOBONamespace>
        <oboInOwl:id>GAZ:00281470</oboInOwl:id>
        <rdfs:label>Taung</rdfs:label>
    </owl:NamedIndividual>
    


    <!-- http://purl.obolibrary.org/obo/GAZ_00281471 -->

    <owl:NamedIndividual rdf:about="http://purl.obolibrary.org/obo/GAZ_00281471">
        <obo:RO_0001025 rdf:resource="http://purl.obolibrary.org/obo/GAZ_00281470"/>
        <obo:IAO_0000115>A paleontological site. A quarry.</obo:IAO_0000115>
        <oboInOwl:hasOBONamespace>GAZ</oboInOwl:hasOBONamespace>
        <oboInOwl:id>GAZ:00281471</oboInOwl:id>
        <rdfs:label>Buxton-limestone quarry</rdfs:label>
    </owl:NamedIndividual>
    


    <!-- http://purl.obolibrary.org/obo/GAZ_00281472 -->

    <owl:NamedIndividual rdf:about="http://purl.obolibrary.org/obo/GAZ_00281472">
        <obo:RO_0001025 rdf:resource="http://purl.obolibrary.org/obo/GAZ_00002812"/>
        <obo:IAO_0000115>A sandstone cliff cave in northern KwaZulu-Natal, South Africa. It is an important Middle Stone Age archeological site.</obo:IAO_0000115>
        <oboInOwl:hasOBONamespace>GAZ</oboInOwl:hasOBONamespace>
        <oboInOwl:id>GAZ:00281472</oboInOwl:id>
        <rdfs:label>Sibudu Cave</rdfs:label>
    </owl:NamedIndividual>
    


    <!-- http://purl.obolibrary.org/obo/GAZ_00281473 -->

    <owl:NamedIndividual rdf:about="http://purl.obolibrary.org/obo/GAZ_00281473">
        <obo:RO_0001025 rdf:resource="http://purl.obolibrary.org/obo/GAZ_00002813"/>
    </owl:NamedIndividual>
    


    <!-- http://purl.obolibrary.org/obo/GAZ_00281475 -->

    <owl:NamedIndividual rdf:about="http://purl.obolibrary.org/obo/GAZ_00281475">
        <obo:RO_0001025 rdf:resource="http://purl.obolibrary.org/obo/GAZ_00281476"/>
        <obo:IAO_0000115>An archeological site. Caves.</obo:IAO_0000115>
        <oboInOwl:hasOBONamespace>GAZ</oboInOwl:hasOBONamespace>
        <oboInOwl:id>GAZ:00281475</oboInOwl:id>
        <rdfs:label>Pinnacle Point [site]</rdfs:label>
    </owl:NamedIndividual>
    


    <!-- http://purl.obolibrary.org/obo/GAZ_00281476 -->

    <owl:NamedIndividual rdf:about="http://purl.obolibrary.org/obo/GAZ_00281476">
        <obo:RO_0001025 rdf:resource="http://purl.obolibrary.org/obo/GAZ_00076130"/>
        <obo:IAO_0000115>A golf course.</obo:IAO_0000115>
        <oboInOwl:hasOBONamespace>GAZ</oboInOwl:hasOBONamespace>
        <oboInOwl:id>GAZ:00281476</oboInOwl:id>
        <rdfs:label>Pinnacle Point [golf course]</rdfs:label>
    </owl:NamedIndividual>
    


    <!-- http://purl.obolibrary.org/obo/GAZ_00281477 -->

    <owl:NamedIndividual rdf:about="http://purl.obolibrary.org/obo/GAZ_00281477">
        <rdf:type rdf:resource="http://purl.obolibrary.org/obo/ENVO_00000191"/>
        <obo:RO_0001025 rdf:resource="http://purl.obolibrary.org/obo/GAZ_00002818"/>
        <obo:IAO_0000115>A geological feature between Kimberley and Barkly West, South Africa, pertaining to the Palaeozoic-age Dwyka Ice Age, or Karoo Ice Age, (some 300 million years ago) where the glacially scoured (smoothed and striated) ancient bedrock (re-exposed by erosion) was used, substantially more recently, during the Later Stone Age period in the late Holocene as panels for rock engravings.</obo:IAO_0000115>
        <oboInOwl:hasOBONamespace>GAZ</oboInOwl:hasOBONamespace>
        <oboInOwl:id>GAZ:00281477</oboInOwl:id>
        <rdfs:label>Nooitgedacht Glacial Pavements</rdfs:label>
    </owl:NamedIndividual>
    


    <!-- http://purl.obolibrary.org/obo/GAZ_00281478 -->

    <owl:NamedIndividual rdf:about="http://purl.obolibrary.org/obo/GAZ_00281478">
        <obo:RO_0001025 rdf:resource="http://purl.obolibrary.org/obo/GAZ_00239595"/>
        <obo:IAO_0000115>A fossil-bearing cave located about 15 km Northeast of Sterkfontein and Swartkrans and about 45 km North-Northwest of the City of Johannesburg, South Africa.</obo:IAO_0000115>
        <oboInOwl:hasOBONamespace>GAZ</oboInOwl:hasOBONamespace>
        <oboInOwl:id>GAZ:00281478</oboInOwl:id>
        <rdfs:label>Malapa Fossil Site</rdfs:label>
    </owl:NamedIndividual>
    


    <!-- http://purl.obolibrary.org/obo/GAZ_00281479 -->

    <owl:NamedIndividual rdf:about="http://purl.obolibrary.org/obo/GAZ_00281479">
        <obo:RO_0001025 rdf:resource="http://purl.obolibrary.org/obo/GAZ_00002814"/>
        <obo:IAO_0000115>A valley located northeast of Potgietersrust in Limpopo province, South Africa. It is an important paleontological site with the local limeworks containing Australopithecus-bearing deposits dating to between 3.0 and 2.6 million years BP.</obo:IAO_0000115>
        <oboInOwl:hasOBONamespace>GAZ</oboInOwl:hasOBONamespace>
        <oboInOwl:id>GAZ:00281479</oboInOwl:id>
        <rdfs:label>Makapansgat Valley</rdfs:label>
    </owl:NamedIndividual>
    


    <!-- http://purl.obolibrary.org/obo/GAZ_00281480 -->

    <owl:NamedIndividual rdf:about="http://purl.obolibrary.org/obo/GAZ_00281480">
        <obo:RO_0001025 rdf:resource="http://purl.obolibrary.org/obo/GAZ_00281479"/>
        <oboInOwl:hasOBONamespace>GAZ</oboInOwl:hasOBONamespace>
        <oboInOwl:id>GAZ:00281480</oboInOwl:id>
        <rdfs:label>Makapansgat limeworks</rdfs:label>
    </owl:NamedIndividual>
    


    <!-- http://purl.obolibrary.org/obo/GAZ_00281481 -->

    <owl:NamedIndividual rdf:about="http://purl.obolibrary.org/obo/GAZ_00281481">
        <obo:RO_0001025 rdf:resource="http://purl.obolibrary.org/obo/GAZ_00281479"/>
        <obo:IAO_0000115>A cave. An archeological site.</obo:IAO_0000115>
        <oboInOwl:hasOBONamespace>GAZ</oboInOwl:hasOBONamespace>
        <oboInOwl:id>GAZ:00281481</oboInOwl:id>
        <rdfs:label>Cave of Hearths</rdfs:label>
    </owl:NamedIndividual>
    


    <!-- http://purl.obolibrary.org/obo/GAZ_00281482 -->

    <owl:NamedIndividual rdf:about="http://purl.obolibrary.org/obo/GAZ_00281482">
        <obo:RO_0001025 rdf:resource="http://purl.obolibrary.org/obo/GAZ_00281479"/>
        <obo:IAO_0000115>A cave. An archeological site.</obo:IAO_0000115>
        <oboInOwl:hasOBONamespace>GAZ</oboInOwl:hasOBONamespace>
        <oboInOwl:id>GAZ:00281482</oboInOwl:id>
        <rdfs:label>Hyaena Mandible Cave</rdfs:label>
    </owl:NamedIndividual>
    


    <!-- http://purl.obolibrary.org/obo/GAZ_00281483 -->

    <owl:NamedIndividual rdf:about="http://purl.obolibrary.org/obo/GAZ_00281483">
        <obo:RO_0001025 rdf:resource="http://purl.obolibrary.org/obo/GAZ_00281479"/>
        <obo:IAO_0000115>A cave. An archeological site.</obo:IAO_0000115>
        <oboInOwl:hasOBONamespace>GAZ</oboInOwl:hasOBONamespace>
        <oboInOwl:id>GAZ:00281483</oboInOwl:id>
        <rdfs:label>Buffalo Cave</rdfs:label>
    </owl:NamedIndividual>
    


    <!-- http://purl.obolibrary.org/obo/GAZ_00281484 -->

    <owl:NamedIndividual rdf:about="http://purl.obolibrary.org/obo/GAZ_00281484">
        <obo:RO_0001025 rdf:resource="http://purl.obolibrary.org/obo/GAZ_00281479"/>
        <obo:IAO_0000115>A cave. An archeological site.</obo:IAO_0000115>
        <oboInOwl:hasOBONamespace>GAZ</oboInOwl:hasOBONamespace>
        <oboInOwl:id>GAZ:00281484</oboInOwl:id>
        <rdfs:label>Ficus Cave and Iron Age Site</rdfs:label>
    </owl:NamedIndividual>
    


    <!-- http://purl.obolibrary.org/obo/GAZ_00281485 -->

    <owl:NamedIndividual rdf:about="http://purl.obolibrary.org/obo/GAZ_00281485">
        <obo:RO_0001025 rdf:resource="http://purl.obolibrary.org/obo/GAZ_00281479"/>
        <obo:IAO_0000115>A cave. An archeological site.</obo:IAO_0000115>
        <oboInOwl:hasOBONamespace>GAZ</oboInOwl:hasOBONamespace>
        <oboInOwl:id>GAZ:00281485</oboInOwl:id>
        <rdfs:label>Katzenjammer Cave</rdfs:label>
    </owl:NamedIndividual>
    


    <!-- http://purl.obolibrary.org/obo/GAZ_00281486 -->

    <owl:NamedIndividual rdf:about="http://purl.obolibrary.org/obo/GAZ_00281486">
        <obo:RO_0001025 rdf:resource="http://purl.obolibrary.org/obo/GAZ_00281479"/>
        <obo:IAO_0000115>A cave. An archeological site.</obo:IAO_0000115>
        <oboInOwl:hasOBONamespace>GAZ</oboInOwl:hasOBONamespace>
        <oboInOwl:id>GAZ:00281486</oboInOwl:id>
        <rdfs:label>Peppercorn&apos;s Cave</rdfs:label>
    </owl:NamedIndividual>
    


    <!-- http://purl.obolibrary.org/obo/GAZ_00281487 -->

    <owl:NamedIndividual rdf:about="http://purl.obolibrary.org/obo/GAZ_00281487">
        <obo:RO_0001025 rdf:resource="http://purl.obolibrary.org/obo/GAZ_00281479"/>
        <obo:IAO_0000115>A cave. An archeological site.</obo:IAO_0000115>
        <oboInOwl:hasOBONamespace>GAZ</oboInOwl:hasOBONamespace>
        <oboInOwl:id>GAZ:00281487</oboInOwl:id>
        <rdfs:label>Rainbow Cave</rdfs:label>
    </owl:NamedIndividual>
    


    <!-- http://purl.obolibrary.org/obo/GAZ_00281488 -->

    <owl:NamedIndividual rdf:about="http://purl.obolibrary.org/obo/GAZ_00281488">
        <obo:RO_0001025 rdf:resource="http://purl.obolibrary.org/obo/GAZ_00281479"/>
        <obo:IAO_0000115>A cave. An archeological site.</obo:IAO_0000115>
        <oboInOwl:hasOBONamespace>GAZ</oboInOwl:hasOBONamespace>
        <oboInOwl:id>GAZ:00281488</oboInOwl:id>
        <rdfs:label>Historic Cave</rdfs:label>
    </owl:NamedIndividual>
    


    <!-- http://purl.obolibrary.org/obo/GAZ_00281489 -->

    <owl:NamedIndividual rdf:about="http://purl.obolibrary.org/obo/GAZ_00281489">
        <obo:RO_0001025 rdf:resource="http://purl.obolibrary.org/obo/GAZ_00281479"/>
        <obo:IAO_0000115>A cave. An archeological site.</obo:IAO_0000115>
        <oboInOwl:hasOBONamespace>GAZ</oboInOwl:hasOBONamespace>
        <oboInOwl:id>GAZ:00281489</oboInOwl:id>
        <rdfs:label>Murzel&apos;s Cave</rdfs:label>
    </owl:NamedIndividual>
    


    <!-- http://purl.obolibrary.org/obo/GAZ_00281490 -->

    <owl:NamedIndividual rdf:about="http://purl.obolibrary.org/obo/GAZ_00281490">
        <obo:RO_0001025 rdf:resource="http://purl.obolibrary.org/obo/GAZ_00281479"/>
        <obo:IAO_0000115>A cave. An archeological site.</obo:IAO_0000115>
        <oboInOwl:hasOBONamespace>GAZ</oboInOwl:hasOBONamespace>
        <oboInOwl:id>GAZ:00281490</oboInOwl:id>
        <rdfs:label>Cold Air Cave</rdfs:label>
    </owl:NamedIndividual>
    


    <!-- http://purl.obolibrary.org/obo/GAZ_00281491 -->

    <owl:NamedIndividual rdf:about="http://purl.obolibrary.org/obo/GAZ_00281491">
        <obo:RO_0001025 rdf:resource="http://purl.obolibrary.org/obo/GAZ_00281479"/>
        <obo:IAO_0000115>A cave. An archeological site.</obo:IAO_0000115>
        <oboInOwl:hasOBONamespace>GAZ</oboInOwl:hasOBONamespace>
        <oboInOwl:id>GAZ:00281491</oboInOwl:id>
        <rdfs:label>Gutentight Cave</rdfs:label>
    </owl:NamedIndividual>
    


    <!-- http://purl.obolibrary.org/obo/GAZ_00281492 -->

    <owl:NamedIndividual rdf:about="http://purl.obolibrary.org/obo/GAZ_00281492">
        <obo:RO_0001025 rdf:resource="http://purl.obolibrary.org/obo/GAZ_00002819"/>
        <obo:IAO_0000115>An archeological site. A small rock cave in South Africa containing the archeological site from which the Howiesons Poort period in the Middle Stone Age gets its name.</obo:IAO_0000115>
        <oboInOwl:hasOBONamespace>GAZ</oboInOwl:hasOBONamespace>
        <oboInOwl:id>GAZ:00281492</oboInOwl:id>
        <rdfs:label>Howieson&apos;s Poort Shelter</rdfs:label>
    </owl:NamedIndividual>
    


    <!-- http://purl.obolibrary.org/obo/GAZ_00281493 -->

    <owl:NamedIndividual rdf:about="http://purl.obolibrary.org/obo/GAZ_00281493">
        <rdf:type rdf:resource="http://purl.obolibrary.org/obo/ENVO_00000305"/>
        <obo:RO_0001025 rdf:resource="http://purl.obolibrary.org/obo/GAZ_00076118"/>
        <obo:IAO_0000115>A headland.</obo:IAO_0000115>
        <oboInOwl:hasOBONamespace>GAZ</oboInOwl:hasOBONamespace>
        <oboInOwl:id>GAZ:00281493</oboInOwl:id>
        <rdfs:label>Hoedjiespunt</rdfs:label>
    </owl:NamedIndividual>
    


    <!-- http://purl.obolibrary.org/obo/GAZ_00281494 -->

    <owl:NamedIndividual rdf:about="http://purl.obolibrary.org/obo/GAZ_00281494">
        <obo:RO_0001025 rdf:resource="http://purl.obolibrary.org/obo/GAZ_00281493"/>
        <obo:IAO_0000115>A paleontological site. A Middle Pleistocene aged hominid fossil-bearing site on the West coast of South Africa, near the town of Saldanha Bay.</obo:IAO_0000115>
        <oboInOwl:hasOBONamespace>GAZ</oboInOwl:hasOBONamespace>
        <oboInOwl:id>GAZ:00281494</oboInOwl:id>
        <rdfs:label>Hoedjiespunt [site]</rdfs:label>
    </owl:NamedIndividual>
    


    <!-- http://purl.obolibrary.org/obo/GAZ_00281495 -->

    <owl:NamedIndividual rdf:about="http://purl.obolibrary.org/obo/GAZ_00281495">
        <obo:RO_0001025 rdf:resource="http://purl.obolibrary.org/obo/GAZ_00002816"/>
        <obo:IAO_0000115>Caves in Precambrian dolomite rock.</obo:IAO_0000115>
        <oboInOwl:hasOBONamespace>GAZ</oboInOwl:hasOBONamespace>
        <oboInOwl:id>GAZ:00281495</oboInOwl:id>
        <rdfs:label>Sudwala Caves</rdfs:label>
    </owl:NamedIndividual>
    


    <!-- http://purl.obolibrary.org/obo/GAZ_00387318 -->

    <owl:NamedIndividual rdf:about="http://purl.obolibrary.org/obo/GAZ_00387318">
        <obo:RO_0001025 rdf:resource="http://purl.obolibrary.org/obo/GAZ_00240244"/>
        <obo:IAO_0000115>A botanical garden.</obo:IAO_0000115>
        <oboInOwl:hasOBONamespace>GAZ</oboInOwl:hasOBONamespace>
        <oboInOwl:id>GAZ:00387318</oboInOwl:id>
        <rdfs:label>Johannesburg Botanical Garden</rdfs:label>
    </owl:NamedIndividual>
    


    <!-- http://purl.obolibrary.org/obo/GAZ_00387319 -->

    <owl:NamedIndividual rdf:about="http://purl.obolibrary.org/obo/GAZ_00387319">
        <obo:RO_0001025 rdf:resource="http://purl.obolibrary.org/obo/GAZ_00239654"/>
        <obo:IAO_0000115>A botanical garden.</obo:IAO_0000115>
        <oboInOwl:hasOBONamespace>GAZ</oboInOwl:hasOBONamespace>
        <oboInOwl:id>GAZ:00387319</oboInOwl:id>
        <rdfs:label>Durban Botanic Gardens</rdfs:label>
    </owl:NamedIndividual>
    


    <!-- http://purl.obolibrary.org/obo/GAZ_00387320 -->

    <owl:NamedIndividual rdf:about="http://purl.obolibrary.org/obo/GAZ_00387320">
        <obo:RO_0001025 rdf:resource="http://purl.obolibrary.org/obo/GAZ_00239618"/>
        <obo:IAO_0000115>A neighborhood of Johannesburg.</obo:IAO_0000115>
        <oboInOwl:hasOBONamespace>GAZ</oboInOwl:hasOBONamespace>
        <oboInOwl:id>GAZ:00387320</oboInOwl:id>
        <rdfs:label>Diepsloot</rdfs:label>
    </owl:NamedIndividual>
    


    <!-- http://purl.obolibrary.org/obo/GAZ_00387321 -->

    <owl:NamedIndividual rdf:about="http://purl.obolibrary.org/obo/GAZ_00387321">
        <obo:RO_0001025 rdf:resource="http://purl.obolibrary.org/obo/GAZ_00239618"/>
        <oboInOwl:hasOBONamespace>GAZ</oboInOwl:hasOBONamespace>
        <oboInOwl:id>GAZ:00387321</oboInOwl:id>
        <rdfs:label>Kya Sand</rdfs:label>
    </owl:NamedIndividual>
    


    <!-- http://purl.obolibrary.org/obo/GAZ_00387322 -->

    <owl:NamedIndividual rdf:about="http://purl.obolibrary.org/obo/GAZ_00387322">
        <obo:RO_0001025 rdf:resource="http://purl.obolibrary.org/obo/GAZ_00239619"/>
        <obo:IAO_0000115>A neighborhood of Johannesburg.</obo:IAO_0000115>
        <oboInOwl:hasOBONamespace>GAZ</oboInOwl:hasOBONamespace>
        <oboInOwl:id>GAZ:00387322</oboInOwl:id>
        <rdfs:label>Randburg</rdfs:label>
    </owl:NamedIndividual>
    


    <!-- http://purl.obolibrary.org/obo/GAZ_00387323 -->

    <owl:NamedIndividual rdf:about="http://purl.obolibrary.org/obo/GAZ_00387323">
        <obo:RO_0001025 rdf:resource="http://purl.obolibrary.org/obo/GAZ_00239619"/>
        <obo:IAO_0000115>A neighborhood of Johannesburg.</obo:IAO_0000115>
        <oboInOwl:hasOBONamespace>GAZ</oboInOwl:hasOBONamespace>
        <oboInOwl:id>GAZ:00387323</oboInOwl:id>
        <rdfs:label>Rosebank</rdfs:label>
    </owl:NamedIndividual>
    


    <!-- http://purl.obolibrary.org/obo/GAZ_00387324 -->

    <owl:NamedIndividual rdf:about="http://purl.obolibrary.org/obo/GAZ_00387324">
        <obo:RO_0001025 rdf:resource="http://purl.obolibrary.org/obo/GAZ_00239619"/>
        <obo:IAO_0000115>A neighborhood of Johannesburg.</obo:IAO_0000115>
        <oboInOwl:hasOBONamespace>GAZ</oboInOwl:hasOBONamespace>
        <oboInOwl:id>GAZ:00387324</oboInOwl:id>
        <rdfs:label>Greenside</rdfs:label>
    </owl:NamedIndividual>
    


    <!-- http://purl.obolibrary.org/obo/GAZ_00387325 -->

    <owl:NamedIndividual rdf:about="http://purl.obolibrary.org/obo/GAZ_00387325">
        <obo:RO_0001025 rdf:resource="http://purl.obolibrary.org/obo/GAZ_00239619"/>
        <obo:IAO_0000115>A neighborhood of Johannesburg.</obo:IAO_0000115>
        <oboInOwl:hasOBONamespace>GAZ</oboInOwl:hasOBONamespace>
        <oboInOwl:id>GAZ:00387325</oboInOwl:id>
        <rdfs:label>Melville</rdfs:label>
    </owl:NamedIndividual>
    


    <!-- http://purl.obolibrary.org/obo/GAZ_00387326 -->

    <owl:NamedIndividual rdf:about="http://purl.obolibrary.org/obo/GAZ_00387326">
        <obo:RO_0001025 rdf:resource="http://purl.obolibrary.org/obo/GAZ_00239619"/>
        <obo:IAO_0000115>A neighborhood of Johannesburg.</obo:IAO_0000115>
        <oboInOwl:hasOBONamespace>GAZ</oboInOwl:hasOBONamespace>
        <oboInOwl:id>GAZ:00387326</oboInOwl:id>
        <rdfs:label>Northcliff</rdfs:label>
    </owl:NamedIndividual>
    


    <!-- http://purl.obolibrary.org/obo/GAZ_00387327 -->

    <owl:NamedIndividual rdf:about="http://purl.obolibrary.org/obo/GAZ_00387327">
        <obo:RO_0001025 rdf:resource="http://purl.obolibrary.org/obo/GAZ_00387330"/>
        <obo:IAO_0000115>A botanical garden.</obo:IAO_0000115>
        <oboInOwl:hasOBONamespace>GAZ</oboInOwl:hasOBONamespace>
        <oboInOwl:id>GAZ:00387327</oboInOwl:id>
        <rdfs:label>Walter Sisulu National Botanical Garden</rdfs:label>
    </owl:NamedIndividual>
    


    <!-- http://purl.obolibrary.org/obo/GAZ_00387328 -->

    <owl:NamedIndividual rdf:about="http://purl.obolibrary.org/obo/GAZ_00387328">
        <obo:RO_0001025 rdf:resource="http://purl.obolibrary.org/obo/GAZ_00239619"/>
        <obo:IAO_0000115>A neighborhood of Johannesburg.</obo:IAO_0000115>
        <oboInOwl:hasOBONamespace>GAZ</oboInOwl:hasOBONamespace>
        <oboInOwl:id>GAZ:00387328</oboInOwl:id>
        <rdfs:label>Parktown</rdfs:label>
    </owl:NamedIndividual>
    


    <!-- http://purl.obolibrary.org/obo/GAZ_00387329 -->

    <owl:NamedIndividual rdf:about="http://purl.obolibrary.org/obo/GAZ_00387329">
        <obo:RO_0001025 rdf:resource="http://purl.obolibrary.org/obo/GAZ_00239619"/>
        <obo:IAO_0000115>A neighborhood of Johannesburg.</obo:IAO_0000115>
        <oboInOwl:hasOBONamespace>GAZ</oboInOwl:hasOBONamespace>
        <oboInOwl:id>GAZ:00387329</oboInOwl:id>
        <rdfs:label>Parktown North</rdfs:label>
    </owl:NamedIndividual>
    


    <!-- http://purl.obolibrary.org/obo/GAZ_00387330 -->

    <owl:NamedIndividual rdf:about="http://purl.obolibrary.org/obo/GAZ_00387330">
        <obo:RO_0001025 rdf:resource="http://purl.obolibrary.org/obo/GAZ_00239620"/>
        <obo:IAO_0000115>A neighborhood of Johannesburg.</obo:IAO_0000115>
        <oboInOwl:hasOBONamespace>GAZ</oboInOwl:hasOBONamespace>
        <oboInOwl:id>GAZ:00387330</oboInOwl:id>
        <rdfs:label>Roodepoort</rdfs:label>
    </owl:NamedIndividual>
    


    <!-- http://purl.obolibrary.org/obo/GAZ_00387331 -->

    <owl:NamedIndividual rdf:about="http://purl.obolibrary.org/obo/GAZ_00387331">
        <obo:RO_0001025 rdf:resource="http://purl.obolibrary.org/obo/GAZ_00239620"/>
        <obo:IAO_0000115>A neighborhood of Johannesburg.</obo:IAO_0000115>
        <oboInOwl:hasOBONamespace>GAZ</oboInOwl:hasOBONamespace>
        <oboInOwl:id>GAZ:00387331</oboInOwl:id>
        <rdfs:label>Constantia Kloof</rdfs:label>
    </owl:NamedIndividual>
    


    <!-- http://purl.obolibrary.org/obo/GAZ_00387332 -->

    <owl:NamedIndividual rdf:about="http://purl.obolibrary.org/obo/GAZ_00387332">
        <obo:RO_0001025 rdf:resource="http://purl.obolibrary.org/obo/GAZ_00239620"/>
        <obo:IAO_0000115>A neighborhood of Johannesburg.</obo:IAO_0000115>
        <oboInOwl:hasOBONamespace>GAZ</oboInOwl:hasOBONamespace>
        <oboInOwl:id>GAZ:00387332</oboInOwl:id>
        <rdfs:label>Northgate</rdfs:label>
    </owl:NamedIndividual>
    


    <!-- http://purl.obolibrary.org/obo/GAZ_00387333 -->

    <owl:NamedIndividual rdf:about="http://purl.obolibrary.org/obo/GAZ_00387333">
        <obo:RO_0001025 rdf:resource="http://purl.obolibrary.org/obo/GAZ_00239621"/>
        <obo:IAO_0000115>A neighborhood of Johannesburg.</obo:IAO_0000115>
        <oboInOwl:hasOBONamespace>GAZ</oboInOwl:hasOBONamespace>
        <oboInOwl:id>GAZ:00387333</oboInOwl:id>
        <rdfs:label>Doornkop</rdfs:label>
    </owl:NamedIndividual>
    


    <!-- http://purl.obolibrary.org/obo/GAZ_00387334 -->

    <owl:NamedIndividual rdf:about="http://purl.obolibrary.org/obo/GAZ_00387334">
        <obo:RO_0001025 rdf:resource="http://purl.obolibrary.org/obo/GAZ_00239621"/>
        <obo:IAO_0000115>A neighborhood of Johannesburg.</obo:IAO_0000115>
        <oboInOwl:hasOBONamespace>GAZ</oboInOwl:hasOBONamespace>
        <oboInOwl:id>GAZ:00387334</oboInOwl:id>
        <rdfs:label>Dobsonville</rdfs:label>
    </owl:NamedIndividual>
    


    <!-- http://purl.obolibrary.org/obo/GAZ_00387335 -->

    <owl:NamedIndividual rdf:about="http://purl.obolibrary.org/obo/GAZ_00387335">
        <obo:RO_0001025 rdf:resource="http://purl.obolibrary.org/obo/GAZ_00239621"/>
        <obo:IAO_0000115>A neighborhood of Johannesburg.</obo:IAO_0000115>
        <oboInOwl:hasOBONamespace>GAZ</oboInOwl:hasOBONamespace>
        <oboInOwl:id>GAZ:00387335</oboInOwl:id>
        <rdfs:label>Protea Glen</rdfs:label>
    </owl:NamedIndividual>
    


    <!-- http://purl.obolibrary.org/obo/GAZ_00387336 -->

    <owl:NamedIndividual rdf:about="http://purl.obolibrary.org/obo/GAZ_00387336">
        <obo:RO_0001025 rdf:resource="http://purl.obolibrary.org/obo/GAZ_00239622"/>
        <obo:IAO_0000115>A neighborhood of Johannesburg.</obo:IAO_0000115>
        <oboInOwl:hasOBONamespace>GAZ</oboInOwl:hasOBONamespace>
        <oboInOwl:id>GAZ:00387336</oboInOwl:id>
        <rdfs:label>Alexandra</rdfs:label>
    </owl:NamedIndividual>
    


    <!-- http://purl.obolibrary.org/obo/GAZ_00387337 -->

    <owl:NamedIndividual rdf:about="http://purl.obolibrary.org/obo/GAZ_00387337">
        <obo:RO_0001025 rdf:resource="http://purl.obolibrary.org/obo/GAZ_00239622"/>
        <obo:IAO_0000115>A neighborhood of Johannesburg.</obo:IAO_0000115>
        <oboInOwl:hasOBONamespace>GAZ</oboInOwl:hasOBONamespace>
        <oboInOwl:id>GAZ:00387337</oboInOwl:id>
        <rdfs:label>Wynberg</rdfs:label>
    </owl:NamedIndividual>
    


    <!-- http://purl.obolibrary.org/obo/GAZ_00387338 -->

    <owl:NamedIndividual rdf:about="http://purl.obolibrary.org/obo/GAZ_00387338">
        <obo:RO_0001025 rdf:resource="http://purl.obolibrary.org/obo/GAZ_00239622"/>
        <obo:IAO_0000115>A neighborhood of Johannesburg.</obo:IAO_0000115>
        <oboInOwl:hasOBONamespace>GAZ</oboInOwl:hasOBONamespace>
        <oboInOwl:id>GAZ:00387338</oboInOwl:id>
        <rdfs:label>Sandton</rdfs:label>
    </owl:NamedIndividual>
    


    <!-- http://purl.obolibrary.org/obo/GAZ_00387339 -->

    <owl:NamedIndividual rdf:about="http://purl.obolibrary.org/obo/GAZ_00387339">
        <obo:RO_0001025 rdf:resource="http://purl.obolibrary.org/obo/GAZ_00239623"/>
        <obo:IAO_0000115>A neighborhood of Johannesburg.</obo:IAO_0000115>
        <oboInOwl:hasOBONamespace>GAZ</oboInOwl:hasOBONamespace>
        <oboInOwl:id>GAZ:00387339</oboInOwl:id>
        <rdfs:label>Inner City</rdfs:label>
    </owl:NamedIndividual>
    


    <!-- http://purl.obolibrary.org/obo/GAZ_00387340 -->

    <owl:NamedIndividual rdf:about="http://purl.obolibrary.org/obo/GAZ_00387340">
        <obo:RO_0001025 rdf:resource="http://purl.obolibrary.org/obo/GAZ_00239624"/>
        <obo:IAO_0000115>A neighborhood of Johannesburg.</obo:IAO_0000115>
        <oboInOwl:hasOBONamespace>GAZ</oboInOwl:hasOBONamespace>
        <oboInOwl:id>GAZ:00387340</oboInOwl:id>
        <rdfs:label>Orange Farm</rdfs:label>
    </owl:NamedIndividual>
    


    <!-- http://purl.obolibrary.org/obo/GAZ_00387341 -->

    <owl:NamedIndividual rdf:about="http://purl.obolibrary.org/obo/GAZ_00387341">
        <obo:RO_0001025 rdf:resource="http://purl.obolibrary.org/obo/GAZ_00239624"/>
        <obo:IAO_0000115>A neighborhood of Johannesburg.</obo:IAO_0000115>
        <oboInOwl:hasOBONamespace>GAZ</oboInOwl:hasOBONamespace>
        <oboInOwl:id>GAZ:00387341</oboInOwl:id>
        <rdfs:label>Ennerdale</rdfs:label>
    </owl:NamedIndividual>
    


    <!-- http://purl.obolibrary.org/obo/GAZ_00387342 -->

    <owl:NamedIndividual rdf:about="http://purl.obolibrary.org/obo/GAZ_00387342">
        <obo:RO_0001025 rdf:resource="http://purl.obolibrary.org/obo/GAZ_00239624"/>
        <obo:IAO_0000115>A neighborhood of Johannesburg.</obo:IAO_0000115>
        <oboInOwl:hasOBONamespace>GAZ</oboInOwl:hasOBONamespace>
        <oboInOwl:id>GAZ:00387342</oboInOwl:id>
        <rdfs:label>Lenasia</rdfs:label>
    </owl:NamedIndividual>
    


    <!-- http://purl.obolibrary.org/obo/GAZ_00387343 -->

    <owl:NamedIndividual rdf:about="http://purl.obolibrary.org/obo/GAZ_00387343">
        <obo:RO_0001025 rdf:resource="http://purl.obolibrary.org/obo/GAZ_00005311"/>
        <obo:IAO_0000115>A botanical garden.</obo:IAO_0000115>
        <oboInOwl:hasOBONamespace>GAZ</oboInOwl:hasOBONamespace>
        <oboInOwl:id>GAZ:00387343</oboInOwl:id>
        <rdfs:label>Pretoria National Botanical Garden</rdfs:label>
    </owl:NamedIndividual>
    


    <!-- http://purl.obolibrary.org/obo/GAZ_00387344 -->

    <owl:NamedIndividual rdf:about="http://purl.obolibrary.org/obo/GAZ_00387344">
        <obo:RO_0001025 rdf:resource="http://purl.obolibrary.org/obo/GAZ_00009436"/>
        <obo:IAO_0000115>A populated place.</obo:IAO_0000115>
        <oboInOwl:hasOBONamespace>GAZ</oboInOwl:hasOBONamespace>
        <oboInOwl:id>GAZ:00387344</oboInOwl:id>
        <rdfs:label>Akasia</rdfs:label>
    </owl:NamedIndividual>
    


    <!-- http://purl.obolibrary.org/obo/GAZ_00387345 -->

    <owl:NamedIndividual rdf:about="http://purl.obolibrary.org/obo/GAZ_00387345">
        <obo:RO_0001025 rdf:resource="http://purl.obolibrary.org/obo/GAZ_00009436"/>
        <obo:IAO_0000115>A populated place.</obo:IAO_0000115>
        <oboInOwl:hasOBONamespace>GAZ</oboInOwl:hasOBONamespace>
        <oboInOwl:id>GAZ:00387345</oboInOwl:id>
        <rdfs:label>Atteridgeville</rdfs:label>
    </owl:NamedIndividual>
    


    <!-- http://purl.obolibrary.org/obo/GAZ_00387346 -->

    <owl:NamedIndividual rdf:about="http://purl.obolibrary.org/obo/GAZ_00387346">
        <obo:RO_0001025 rdf:resource="http://purl.obolibrary.org/obo/GAZ_00009436"/>
        <obo:IAO_0000115>A populated place.</obo:IAO_0000115>
        <oboInOwl:hasOBONamespace>GAZ</oboInOwl:hasOBONamespace>
        <oboInOwl:id>GAZ:00387346</oboInOwl:id>
        <rdfs:label>Centurion</rdfs:label>
    </owl:NamedIndividual>
    


    <!-- http://purl.obolibrary.org/obo/GAZ_00387347 -->

    <owl:NamedIndividual rdf:about="http://purl.obolibrary.org/obo/GAZ_00387347">
        <obo:RO_0001025 rdf:resource="http://purl.obolibrary.org/obo/GAZ_00009436"/>
        <obo:IAO_0000115>A populated place.</obo:IAO_0000115>
        <oboInOwl:hasOBONamespace>GAZ</oboInOwl:hasOBONamespace>
        <oboInOwl:id>GAZ:00387347</oboInOwl:id>
        <rdfs:label>Crocodile River</rdfs:label>
    </owl:NamedIndividual>
    


    <!-- http://purl.obolibrary.org/obo/GAZ_00387348 -->

    <owl:NamedIndividual rdf:about="http://purl.obolibrary.org/obo/GAZ_00387348">
        <obo:RO_0001025 rdf:resource="http://purl.obolibrary.org/obo/GAZ_00009436"/>
        <obo:IAO_0000115>A populated place.</obo:IAO_0000115>
        <oboInOwl:hasOBONamespace>GAZ</oboInOwl:hasOBONamespace>
        <oboInOwl:id>GAZ:00387348</oboInOwl:id>
        <rdfs:label>Eersterust</rdfs:label>
    </owl:NamedIndividual>
    


    <!-- http://purl.obolibrary.org/obo/GAZ_00387349 -->

    <owl:NamedIndividual rdf:about="http://purl.obolibrary.org/obo/GAZ_00387349">
        <obo:RO_0001025 rdf:resource="http://purl.obolibrary.org/obo/GAZ_00009436"/>
        <obo:IAO_0000115>A populated place.</obo:IAO_0000115>
        <oboInOwl:hasOBONamespace>GAZ</oboInOwl:hasOBONamespace>
        <oboInOwl:id>GAZ:00387349</oboInOwl:id>
        <rdfs:label>Ga-Rankuwa</rdfs:label>
    </owl:NamedIndividual>
    


    <!-- http://purl.obolibrary.org/obo/GAZ_00387350 -->

    <owl:NamedIndividual rdf:about="http://purl.obolibrary.org/obo/GAZ_00387350">
        <obo:RO_0001025 rdf:resource="http://purl.obolibrary.org/obo/GAZ_00009436"/>
        <obo:IAO_0000115>A populated place.</obo:IAO_0000115>
        <oboInOwl:hasOBONamespace>GAZ</oboInOwl:hasOBONamespace>
        <oboInOwl:id>GAZ:00387350</oboInOwl:id>
        <rdfs:label>Hammanskraal</rdfs:label>
    </owl:NamedIndividual>
    


    <!-- http://purl.obolibrary.org/obo/GAZ_00387351 -->

    <owl:NamedIndividual rdf:about="http://purl.obolibrary.org/obo/GAZ_00387351">
        <obo:RO_0001025 rdf:resource="http://purl.obolibrary.org/obo/GAZ_00009436"/>
        <obo:IAO_0000115>A populated place.</obo:IAO_0000115>
        <oboInOwl:hasOBONamespace>GAZ</oboInOwl:hasOBONamespace>
        <oboInOwl:id>GAZ:00387351</oboInOwl:id>
        <rdfs:label>Laudium</rdfs:label>
    </owl:NamedIndividual>
    


    <!-- http://purl.obolibrary.org/obo/GAZ_00387352 -->

    <owl:NamedIndividual rdf:about="http://purl.obolibrary.org/obo/GAZ_00387352">
        <obo:RO_0001025 rdf:resource="http://purl.obolibrary.org/obo/GAZ_00009436"/>
        <obo:IAO_0000115>A populated place.</obo:IAO_0000115>
        <oboInOwl:hasOBONamespace>GAZ</oboInOwl:hasOBONamespace>
        <oboInOwl:id>GAZ:00387352</oboInOwl:id>
        <rdfs:label>Mabopane</rdfs:label>
    </owl:NamedIndividual>
    


    <!-- http://purl.obolibrary.org/obo/GAZ_00387353 -->

    <owl:NamedIndividual rdf:about="http://purl.obolibrary.org/obo/GAZ_00387353">
        <obo:RO_0001025 rdf:resource="http://purl.obolibrary.org/obo/GAZ_00009436"/>
        <obo:IAO_0000115>A populated place.</obo:IAO_0000115>
        <oboInOwl:hasOBONamespace>GAZ</oboInOwl:hasOBONamespace>
        <oboInOwl:id>GAZ:00387353</oboInOwl:id>
        <rdfs:label>Mamelodi</rdfs:label>
    </owl:NamedIndividual>
    


    <!-- http://purl.obolibrary.org/obo/GAZ_00387354 -->

    <owl:NamedIndividual rdf:about="http://purl.obolibrary.org/obo/GAZ_00387354">
        <obo:RO_0001025 rdf:resource="http://purl.obolibrary.org/obo/GAZ_00009436"/>
        <obo:IAO_0000115>A populated place.</obo:IAO_0000115>
        <oboInOwl:hasOBONamespace>GAZ</oboInOwl:hasOBONamespace>
        <oboInOwl:id>GAZ:00387354</oboInOwl:id>
        <rdfs:label>Pienaarsrivier</rdfs:label>
    </owl:NamedIndividual>
    


    <!-- http://purl.obolibrary.org/obo/GAZ_00387355 -->

    <owl:NamedIndividual rdf:about="http://purl.obolibrary.org/obo/GAZ_00387355">
        <obo:RO_0001025 rdf:resource="http://purl.obolibrary.org/obo/GAZ_00009436"/>
        <obo:IAO_0000115>A populated place.</obo:IAO_0000115>
        <oboInOwl:hasOBONamespace>GAZ</oboInOwl:hasOBONamespace>
        <oboInOwl:id>GAZ:00387355</oboInOwl:id>
        <rdfs:label>Soshanguve</rdfs:label>
    </owl:NamedIndividual>
    


    <!-- http://purl.obolibrary.org/obo/GAZ_00387356 -->

    <owl:NamedIndividual rdf:about="http://purl.obolibrary.org/obo/GAZ_00387356">
        <obo:RO_0001025 rdf:resource="http://purl.obolibrary.org/obo/GAZ_00009436"/>
        <obo:IAO_0000115>A populated place.</obo:IAO_0000115>
        <oboInOwl:hasOBONamespace>GAZ</oboInOwl:hasOBONamespace>
        <oboInOwl:id>GAZ:00387356</oboInOwl:id>
        <rdfs:label>Temba</rdfs:label>
    </owl:NamedIndividual>
    


    <!-- http://purl.obolibrary.org/obo/GAZ_00387357 -->

    <owl:NamedIndividual rdf:about="http://purl.obolibrary.org/obo/GAZ_00387357">
        <obo:RO_0001025 rdf:resource="http://purl.obolibrary.org/obo/GAZ_00009436"/>
        <obo:IAO_0000115>A populated place.</obo:IAO_0000115>
        <oboInOwl:hasOBONamespace>GAZ</oboInOwl:hasOBONamespace>
        <oboInOwl:id>GAZ:00387357</oboInOwl:id>
        <rdfs:label>Winterveld</rdfs:label>
    </owl:NamedIndividual>
    


    <!-- http://purl.obolibrary.org/obo/GAZ_00387358 -->

    <owl:NamedIndividual rdf:about="http://purl.obolibrary.org/obo/GAZ_00387358">
        <obo:RO_0001025 rdf:resource="http://purl.obolibrary.org/obo/GAZ_00387355"/>
        <obo:IAO_0000115>An impact crater (astrobleme). Contains a lake.</obo:IAO_0000115>
        <oboInOwl:hasOBONamespace>GAZ</oboInOwl:hasOBONamespace>
        <oboInOwl:id>GAZ:00387358</oboInOwl:id>
        <rdfs:label>Tswaing crater</rdfs:label>
    </owl:NamedIndividual>
    


    <!-- http://purl.obolibrary.org/obo/GAZ_00387360 -->

    <owl:NamedIndividual rdf:about="http://purl.obolibrary.org/obo/GAZ_00387360">
        <obo:RO_0001025 rdf:resource="http://purl.obolibrary.org/obo/GAZ_00076003"/>
        <obo:IAO_0000115>A populated place.</obo:IAO_0000115>
        <oboInOwl:hasOBONamespace>GAZ</oboInOwl:hasOBONamespace>
        <oboInOwl:id>GAZ:00387360</oboInOwl:id>
        <rdfs:label>Bloemfontein</rdfs:label>
    </owl:NamedIndividual>
    


    <!-- http://purl.obolibrary.org/obo/GAZ_00387361 -->

    <owl:NamedIndividual rdf:about="http://purl.obolibrary.org/obo/GAZ_00387361">
        <obo:RO_0001025 rdf:resource="http://purl.obolibrary.org/obo/GAZ_00387360"/>
        <obo:IAO_0000115>A botanical garden.</obo:IAO_0000115>
        <oboInOwl:hasOBONamespace>GAZ</oboInOwl:hasOBONamespace>
        <oboInOwl:id>GAZ:00387361</oboInOwl:id>
        <rdfs:label>Free State National Botanical Garden</rdfs:label>
    </owl:NamedIndividual>
    


    <!-- http://purl.obolibrary.org/obo/GAZ_00387362 -->

    <owl:NamedIndividual rdf:about="http://purl.obolibrary.org/obo/GAZ_00387362">
        <obo:RO_0001025 rdf:resource="http://purl.obolibrary.org/obo/GAZ_00387374"/>
        <obo:IAO_0000115>A botanical garden.</obo:IAO_0000115>
        <oboInOwl:hasOBONamespace>GAZ</oboInOwl:hasOBONamespace>
        <oboInOwl:id>GAZ:00387362</oboInOwl:id>
        <rdfs:label>Harold Porter National Botanical Garden</rdfs:label>
    </owl:NamedIndividual>
    


    <!-- http://purl.obolibrary.org/obo/GAZ_00387363 -->

    <owl:NamedIndividual rdf:about="http://purl.obolibrary.org/obo/GAZ_00387363">
        <obo:RO_0001025 rdf:resource="http://purl.obolibrary.org/obo/GAZ_00076085"/>
        <obo:IAO_0000115>A populated place.</obo:IAO_0000115>
        <oboInOwl:hasOBONamespace>GAZ</oboInOwl:hasOBONamespace>
        <oboInOwl:id>GAZ:00387363</oboInOwl:id>
        <rdfs:label>Brandvlei</rdfs:label>
    </owl:NamedIndividual>
    


    <!-- http://purl.obolibrary.org/obo/GAZ_00387364 -->

    <owl:NamedIndividual rdf:about="http://purl.obolibrary.org/obo/GAZ_00387364">
        <obo:RO_0001025 rdf:resource="http://purl.obolibrary.org/obo/GAZ_00076085"/>
        <obo:IAO_0000115>A populated place.</obo:IAO_0000115>
        <oboInOwl:hasOBONamespace>GAZ</oboInOwl:hasOBONamespace>
        <oboInOwl:id>GAZ:00387364</oboInOwl:id>
        <rdfs:label>Calvinia</rdfs:label>
    </owl:NamedIndividual>
    


    <!-- http://purl.obolibrary.org/obo/GAZ_00387365 -->

    <owl:NamedIndividual rdf:about="http://purl.obolibrary.org/obo/GAZ_00387365">
        <obo:RO_0001025 rdf:resource="http://purl.obolibrary.org/obo/GAZ_00076085"/>
        <obo:IAO_0000115>A populated place.</obo:IAO_0000115>
        <oboInOwl:hasOBONamespace>GAZ</oboInOwl:hasOBONamespace>
        <oboInOwl:id>GAZ:00387365</oboInOwl:id>
        <rdfs:label>Fraserburg</rdfs:label>
    </owl:NamedIndividual>
    


    <!-- http://purl.obolibrary.org/obo/GAZ_00387366 -->

    <owl:NamedIndividual rdf:about="http://purl.obolibrary.org/obo/GAZ_00387366">
        <obo:RO_0001025 rdf:resource="http://purl.obolibrary.org/obo/GAZ_00076085"/>
        <obo:IAO_0000115>A populated place.</obo:IAO_0000115>
        <oboInOwl:hasOBONamespace>GAZ</oboInOwl:hasOBONamespace>
        <oboInOwl:id>GAZ:00387366</oboInOwl:id>
        <rdfs:label>Loeriesfontein</rdfs:label>
    </owl:NamedIndividual>
    


    <!-- http://purl.obolibrary.org/obo/GAZ_00387367 -->

    <owl:NamedIndividual rdf:about="http://purl.obolibrary.org/obo/GAZ_00387367">
        <obo:RO_0001025 rdf:resource="http://purl.obolibrary.org/obo/GAZ_00076085"/>
        <obo:IAO_0000115>A populated place.</obo:IAO_0000115>
        <oboInOwl:hasOBONamespace>GAZ</oboInOwl:hasOBONamespace>
        <oboInOwl:id>GAZ:00387367</oboInOwl:id>
        <rdfs:label>Nieuwoudtville</rdfs:label>
    </owl:NamedIndividual>
    


    <!-- http://purl.obolibrary.org/obo/GAZ_00387368 -->

    <owl:NamedIndividual rdf:about="http://purl.obolibrary.org/obo/GAZ_00387368">
        <obo:RO_0001025 rdf:resource="http://purl.obolibrary.org/obo/GAZ_00076085"/>
        <obo:IAO_0000115>A populated place.</obo:IAO_0000115>
        <oboInOwl:hasOBONamespace>GAZ</oboInOwl:hasOBONamespace>
        <oboInOwl:id>GAZ:00387368</oboInOwl:id>
        <rdfs:label>Nuwepos</rdfs:label>
    </owl:NamedIndividual>
    


    <!-- http://purl.obolibrary.org/obo/GAZ_00387369 -->

    <owl:NamedIndividual rdf:about="http://purl.obolibrary.org/obo/GAZ_00387369">
        <obo:RO_0001025 rdf:resource="http://purl.obolibrary.org/obo/GAZ_00076085"/>
        <obo:IAO_0000115>A populated place.</obo:IAO_0000115>
        <oboInOwl:hasOBONamespace>GAZ</oboInOwl:hasOBONamespace>
        <oboInOwl:id>GAZ:00387369</oboInOwl:id>
        <rdfs:label>Sutherland</rdfs:label>
    </owl:NamedIndividual>
    


    <!-- http://purl.obolibrary.org/obo/GAZ_00387370 -->

    <owl:NamedIndividual rdf:about="http://purl.obolibrary.org/obo/GAZ_00387370">
        <obo:RO_0001025 rdf:resource="http://purl.obolibrary.org/obo/GAZ_00076085"/>
        <obo:IAO_0000115>A populated place.</obo:IAO_0000115>
        <oboInOwl:hasOBONamespace>GAZ</oboInOwl:hasOBONamespace>
        <oboInOwl:id>GAZ:00387370</oboInOwl:id>
        <rdfs:label>Vanwyksvlei</rdfs:label>
    </owl:NamedIndividual>
    


    <!-- http://purl.obolibrary.org/obo/GAZ_00387371 -->

    <owl:NamedIndividual rdf:about="http://purl.obolibrary.org/obo/GAZ_00387371">
        <obo:RO_0001025 rdf:resource="http://purl.obolibrary.org/obo/GAZ_00076085"/>
        <obo:IAO_0000115>A populated place.</obo:IAO_0000115>
        <oboInOwl:hasOBONamespace>GAZ</oboInOwl:hasOBONamespace>
        <oboInOwl:id>GAZ:00387371</oboInOwl:id>
        <rdfs:label>Williston</rdfs:label>
    </owl:NamedIndividual>
    


    <!-- http://purl.obolibrary.org/obo/GAZ_00387372 -->

    <owl:NamedIndividual rdf:about="http://purl.obolibrary.org/obo/GAZ_00387372">
        <obo:RO_0001025 rdf:resource="http://purl.obolibrary.org/obo/GAZ_00387367"/>
        <obo:IAO_0000115>A botanical garden.</obo:IAO_0000115>
        <oboInOwl:hasOBONamespace>GAZ</oboInOwl:hasOBONamespace>
        <oboInOwl:id>GAZ:00387372</oboInOwl:id>
        <rdfs:label>Hantam National Botanical Garden</rdfs:label>
    </owl:NamedIndividual>
    


    <!-- http://purl.obolibrary.org/obo/GAZ_00387373 -->

    <owl:NamedIndividual rdf:about="http://purl.obolibrary.org/obo/GAZ_00387373">
        <obo:RO_0001025 rdf:resource="http://purl.obolibrary.org/obo/GAZ_00076123"/>
        <obo:IAO_0000115>A populated place.</obo:IAO_0000115>
        <oboInOwl:hasOBONamespace>GAZ</oboInOwl:hasOBONamespace>
        <oboInOwl:id>GAZ:00387373</oboInOwl:id>
        <rdfs:label>Baardskeerdersbos</rdfs:label>
    </owl:NamedIndividual>
    


    <!-- http://purl.obolibrary.org/obo/GAZ_00387374 -->

    <owl:NamedIndividual rdf:about="http://purl.obolibrary.org/obo/GAZ_00387374">
        <obo:RO_0001025 rdf:resource="http://purl.obolibrary.org/obo/GAZ_00076123"/>
        <obo:IAO_0000115>A populated place.</obo:IAO_0000115>
        <oboInOwl:hasOBONamespace>GAZ</oboInOwl:hasOBONamespace>
        <oboInOwl:id>GAZ:00387374</oboInOwl:id>
        <rdfs:label>Bettys Bay</rdfs:label>
    </owl:NamedIndividual>
    


    <!-- http://purl.obolibrary.org/obo/GAZ_00387375 -->

    <owl:NamedIndividual rdf:about="http://purl.obolibrary.org/obo/GAZ_00387375">
        <obo:RO_0001025 rdf:resource="http://purl.obolibrary.org/obo/GAZ_00076123"/>
        <obo:IAO_0000115>A populated place.</obo:IAO_0000115>
        <oboInOwl:hasOBONamespace>GAZ</oboInOwl:hasOBONamespace>
        <oboInOwl:id>GAZ:00387375</oboInOwl:id>
        <rdfs:label>Die Kelders</rdfs:label>
    </owl:NamedIndividual>
    


    <!-- http://purl.obolibrary.org/obo/GAZ_00387376 -->

    <owl:NamedIndividual rdf:about="http://purl.obolibrary.org/obo/GAZ_00387376">
        <obo:RO_0001025 rdf:resource="http://purl.obolibrary.org/obo/GAZ_00076123"/>
        <obo:IAO_0000115>A populated place.</obo:IAO_0000115>
        <oboInOwl:hasOBONamespace>GAZ</oboInOwl:hasOBONamespace>
        <oboInOwl:id>GAZ:00387376</oboInOwl:id>
        <rdfs:label>Fisherhaven</rdfs:label>
    </owl:NamedIndividual>
    


    <!-- http://purl.obolibrary.org/obo/GAZ_00387377 -->

    <owl:NamedIndividual rdf:about="http://purl.obolibrary.org/obo/GAZ_00387377">
        <obo:RO_0001025 rdf:resource="http://purl.obolibrary.org/obo/GAZ_00076123"/>
        <obo:IAO_0000115>A populated place.</obo:IAO_0000115>
        <oboInOwl:hasOBONamespace>GAZ</oboInOwl:hasOBONamespace>
        <oboInOwl:id>GAZ:00387377</oboInOwl:id>
        <rdfs:label>Franskraalstrand</rdfs:label>
    </owl:NamedIndividual>
    


    <!-- http://purl.obolibrary.org/obo/GAZ_00387378 -->

    <owl:NamedIndividual rdf:about="http://purl.obolibrary.org/obo/GAZ_00387378">
        <obo:RO_0001025 rdf:resource="http://purl.obolibrary.org/obo/GAZ_00076123"/>
        <obo:IAO_0000115>A populated place.</obo:IAO_0000115>
        <oboInOwl:hasOBONamespace>GAZ</oboInOwl:hasOBONamespace>
        <oboInOwl:id>GAZ:00387378</oboInOwl:id>
        <rdfs:label>Gansbaai</rdfs:label>
    </owl:NamedIndividual>
    


    <!-- http://purl.obolibrary.org/obo/GAZ_00387379 -->

    <owl:NamedIndividual rdf:about="http://purl.obolibrary.org/obo/GAZ_00387379">
        <obo:RO_0001025 rdf:resource="http://purl.obolibrary.org/obo/GAZ_00076123"/>
        <obo:IAO_0000115>A populated place.</obo:IAO_0000115>
        <oboInOwl:hasOBONamespace>GAZ</oboInOwl:hasOBONamespace>
        <oboInOwl:id>GAZ:00387379</oboInOwl:id>
        <rdfs:label>Hawston</rdfs:label>
    </owl:NamedIndividual>
    


    <!-- http://purl.obolibrary.org/obo/GAZ_00387380 -->

    <owl:NamedIndividual rdf:about="http://purl.obolibrary.org/obo/GAZ_00387380">
        <obo:RO_0001025 rdf:resource="http://purl.obolibrary.org/obo/GAZ_00076123"/>
        <obo:IAO_0000115>A populated place.</obo:IAO_0000115>
        <oboInOwl:hasOBONamespace>GAZ</oboInOwl:hasOBONamespace>
        <oboInOwl:id>GAZ:00387380</oboInOwl:id>
        <rdfs:label>Hermanus</rdfs:label>
    </owl:NamedIndividual>
    


    <!-- http://purl.obolibrary.org/obo/GAZ_00387381 -->

    <owl:NamedIndividual rdf:about="http://purl.obolibrary.org/obo/GAZ_00387381">
        <obo:RO_0001025 rdf:resource="http://purl.obolibrary.org/obo/GAZ_00076123"/>
        <obo:IAO_0000115>A populated place.</obo:IAO_0000115>
        <oboInOwl:hasOBONamespace>GAZ</oboInOwl:hasOBONamespace>
        <oboInOwl:id>GAZ:00387381</oboInOwl:id>
        <rdfs:label>Kleinbaai</rdfs:label>
    </owl:NamedIndividual>
    


    <!-- http://purl.obolibrary.org/obo/GAZ_00387382 -->

    <owl:NamedIndividual rdf:about="http://purl.obolibrary.org/obo/GAZ_00387382">
        <obo:RO_0001025 rdf:resource="http://purl.obolibrary.org/obo/GAZ_00076123"/>
        <obo:IAO_0000115>A populated place.</obo:IAO_0000115>
        <oboInOwl:hasOBONamespace>GAZ</oboInOwl:hasOBONamespace>
        <oboInOwl:id>GAZ:00387382</oboInOwl:id>
        <rdfs:label>Kleinmond</rdfs:label>
    </owl:NamedIndividual>
    


    <!-- http://purl.obolibrary.org/obo/GAZ_00387383 -->

    <owl:NamedIndividual rdf:about="http://purl.obolibrary.org/obo/GAZ_00387383">
        <obo:RO_0001025 rdf:resource="http://purl.obolibrary.org/obo/GAZ_00076123"/>
        <obo:IAO_0000115>A populated place.</obo:IAO_0000115>
        <oboInOwl:hasOBONamespace>GAZ</oboInOwl:hasOBONamespace>
        <oboInOwl:id>GAZ:00387383</oboInOwl:id>
        <rdfs:label>Onrus</rdfs:label>
    </owl:NamedIndividual>
    


    <!-- http://purl.obolibrary.org/obo/GAZ_00387384 -->

    <owl:NamedIndividual rdf:about="http://purl.obolibrary.org/obo/GAZ_00387384">
        <obo:RO_0001025 rdf:resource="http://purl.obolibrary.org/obo/GAZ_00076123"/>
        <obo:IAO_0000115>A populated place.</obo:IAO_0000115>
        <oboInOwl:hasOBONamespace>GAZ</oboInOwl:hasOBONamespace>
        <oboInOwl:id>GAZ:00387384</oboInOwl:id>
        <rdfs:label>Pearly Beach</rdfs:label>
    </owl:NamedIndividual>
    


    <!-- http://purl.obolibrary.org/obo/GAZ_00387385 -->

    <owl:NamedIndividual rdf:about="http://purl.obolibrary.org/obo/GAZ_00387385">
        <obo:RO_0001025 rdf:resource="http://purl.obolibrary.org/obo/GAZ_00076123"/>
        <obo:IAO_0000115>A populated place.</obo:IAO_0000115>
        <oboInOwl:hasOBONamespace>GAZ</oboInOwl:hasOBONamespace>
        <oboInOwl:id>GAZ:00387385</oboInOwl:id>
        <rdfs:label>Pringle Bay</rdfs:label>
    </owl:NamedIndividual>
    


    <!-- http://purl.obolibrary.org/obo/GAZ_00387386 -->

    <owl:NamedIndividual rdf:about="http://purl.obolibrary.org/obo/GAZ_00387386">
        <obo:RO_0001025 rdf:resource="http://purl.obolibrary.org/obo/GAZ_00076123"/>
        <obo:IAO_0000115>A populated place.</obo:IAO_0000115>
        <oboInOwl:hasOBONamespace>GAZ</oboInOwl:hasOBONamespace>
        <oboInOwl:id>GAZ:00387386</oboInOwl:id>
        <rdfs:label>Rooiels</rdfs:label>
    </owl:NamedIndividual>
    


    <!-- http://purl.obolibrary.org/obo/GAZ_00387387 -->

    <owl:NamedIndividual rdf:about="http://purl.obolibrary.org/obo/GAZ_00387387">
        <obo:RO_0001025 rdf:resource="http://purl.obolibrary.org/obo/GAZ_00076123"/>
        <obo:IAO_0000115>A populated place.</obo:IAO_0000115>
        <oboInOwl:hasOBONamespace>GAZ</oboInOwl:hasOBONamespace>
        <oboInOwl:id>GAZ:00387387</oboInOwl:id>
        <rdfs:label>Sandbaai</rdfs:label>
    </owl:NamedIndividual>
    


    <!-- http://purl.obolibrary.org/obo/GAZ_00387388 -->

    <owl:NamedIndividual rdf:about="http://purl.obolibrary.org/obo/GAZ_00387388">
        <obo:RO_0001025 rdf:resource="http://purl.obolibrary.org/obo/GAZ_00076123"/>
        <obo:IAO_0000115>A populated place.</obo:IAO_0000115>
        <oboInOwl:hasOBONamespace>GAZ</oboInOwl:hasOBONamespace>
        <oboInOwl:id>GAZ:00387388</oboInOwl:id>
        <rdfs:label>Silver Sands</rdfs:label>
    </owl:NamedIndividual>
    


    <!-- http://purl.obolibrary.org/obo/GAZ_00387389 -->

    <owl:NamedIndividual rdf:about="http://purl.obolibrary.org/obo/GAZ_00387389">
        <obo:RO_0001025 rdf:resource="http://purl.obolibrary.org/obo/GAZ_00076123"/>
        <obo:IAO_0000115>A populated place.</obo:IAO_0000115>
        <oboInOwl:hasOBONamespace>GAZ</oboInOwl:hasOBONamespace>
        <oboInOwl:id>GAZ:00387389</oboInOwl:id>
        <rdfs:label>Stanford</rdfs:label>
    </owl:NamedIndividual>
    


    <!-- http://purl.obolibrary.org/obo/GAZ_00387390 -->

    <owl:NamedIndividual rdf:about="http://purl.obolibrary.org/obo/GAZ_00387390">
        <obo:RO_0001025 rdf:resource="http://purl.obolibrary.org/obo/GAZ_00076123"/>
        <obo:IAO_0000115>A populated place.</obo:IAO_0000115>
        <oboInOwl:hasOBONamespace>GAZ</oboInOwl:hasOBONamespace>
        <oboInOwl:id>GAZ:00387390</oboInOwl:id>
        <rdfs:label>Uilenkraalsmond</rdfs:label>
    </owl:NamedIndividual>
    


    <!-- http://purl.obolibrary.org/obo/GAZ_00387391 -->

    <owl:NamedIndividual rdf:about="http://purl.obolibrary.org/obo/GAZ_00387391">
        <obo:RO_0001025 rdf:resource="http://purl.obolibrary.org/obo/GAZ_00076123"/>
        <obo:IAO_0000115>A populated place.</obo:IAO_0000115>
        <oboInOwl:hasOBONamespace>GAZ</oboInOwl:hasOBONamespace>
        <oboInOwl:id>GAZ:00387391</oboInOwl:id>
        <rdfs:label>Vermont</rdfs:label>
    </owl:NamedIndividual>
    


    <!-- http://purl.obolibrary.org/obo/GAZ_00387392 -->

    <owl:NamedIndividual rdf:about="http://purl.obolibrary.org/obo/GAZ_00387392">
        <obo:RO_0001025 rdf:resource="http://purl.obolibrary.org/obo/GAZ_00076123"/>
        <obo:IAO_0000115>A populated place.</obo:IAO_0000115>
        <oboInOwl:hasOBONamespace>GAZ</oboInOwl:hasOBONamespace>
        <oboInOwl:id>GAZ:00387392</oboInOwl:id>
        <rdfs:label>Viljoenshof</rdfs:label>
    </owl:NamedIndividual>
    


    <!-- http://purl.obolibrary.org/obo/GAZ_00387393 -->

    <owl:NamedIndividual rdf:about="http://purl.obolibrary.org/obo/GAZ_00387393">
        <obo:RO_0001025 rdf:resource="http://purl.obolibrary.org/obo/GAZ_00076123"/>
        <obo:IAO_0000115>A populated place.</obo:IAO_0000115>
        <oboInOwl:hasOBONamespace>GAZ</oboInOwl:hasOBONamespace>
        <oboInOwl:id>GAZ:00387393</oboInOwl:id>
        <rdfs:label>Voelklip</rdfs:label>
    </owl:NamedIndividual>
    


    <!-- http://purl.obolibrary.org/obo/GAZ_00387394 -->

    <owl:NamedIndividual rdf:about="http://purl.obolibrary.org/obo/GAZ_00387394">
        <obo:RO_0001025 rdf:resource="http://purl.obolibrary.org/obo/GAZ_00076122"/>
        <obo:IAO_0000115>A populated place.</obo:IAO_0000115>
        <oboInOwl:hasOBONamespace>GAZ</oboInOwl:hasOBONamespace>
        <oboInOwl:id>GAZ:00387394</oboInOwl:id>
        <rdfs:label>De Doorns</rdfs:label>
    </owl:NamedIndividual>
    


    <!-- http://purl.obolibrary.org/obo/GAZ_00387395 -->

    <owl:NamedIndividual rdf:about="http://purl.obolibrary.org/obo/GAZ_00387395">
        <obo:RO_0001025 rdf:resource="http://purl.obolibrary.org/obo/GAZ_00076122"/>
        <obo:IAO_0000115>A populated place.</obo:IAO_0000115>
        <oboInOwl:hasOBONamespace>GAZ</oboInOwl:hasOBONamespace>
        <oboInOwl:id>GAZ:00387395</oboInOwl:id>
        <rdfs:label>Rawsonville</rdfs:label>
    </owl:NamedIndividual>
    


    <!-- http://purl.obolibrary.org/obo/GAZ_00387396 -->

    <owl:NamedIndividual rdf:about="http://purl.obolibrary.org/obo/GAZ_00387396">
        <obo:RO_0001025 rdf:resource="http://purl.obolibrary.org/obo/GAZ_00076122"/>
        <obo:IAO_0000115>A populated place.</obo:IAO_0000115>
        <oboInOwl:hasOBONamespace>GAZ</oboInOwl:hasOBONamespace>
        <oboInOwl:id>GAZ:00387396</oboInOwl:id>
        <rdfs:label>Touws River</rdfs:label>
    </owl:NamedIndividual>
    


    <!-- http://purl.obolibrary.org/obo/GAZ_00387397 -->

    <owl:NamedIndividual rdf:about="http://purl.obolibrary.org/obo/GAZ_00387397">
        <obo:RO_0001025 rdf:resource="http://purl.obolibrary.org/obo/GAZ_00076122"/>
        <obo:IAO_0000115>A populated place.</obo:IAO_0000115>
        <oboInOwl:hasOBONamespace>GAZ</oboInOwl:hasOBONamespace>
        <oboInOwl:id>GAZ:00387397</oboInOwl:id>
        <rdfs:label>Worcester</rdfs:label>
    </owl:NamedIndividual>
    


    <!-- http://purl.obolibrary.org/obo/GAZ_00387398 -->

    <owl:NamedIndividual rdf:about="http://purl.obolibrary.org/obo/GAZ_00387398">
        <obo:RO_0001025 rdf:resource="http://purl.obolibrary.org/obo/GAZ_00387397"/>
        <obo:IAO_0000115>A botanical garden.</obo:IAO_0000115>
        <oboInOwl:hasOBONamespace>GAZ</oboInOwl:hasOBONamespace>
        <oboInOwl:id>GAZ:00387398</oboInOwl:id>
        <rdfs:label>Karoo Desert National Botanical Garden</rdfs:label>
    </owl:NamedIndividual>
    


    <!-- http://purl.obolibrary.org/obo/GAZ_00387399 -->

    <owl:NamedIndividual rdf:about="http://purl.obolibrary.org/obo/GAZ_00387399">
        <obo:RO_0001025 rdf:resource="http://purl.obolibrary.org/obo/GAZ_00008041"/>
        <obo:IAO_0000115>A botanical garden.</obo:IAO_0000115>
        <oboInOwl:hasOBONamespace>GAZ</oboInOwl:hasOBONamespace>
        <oboInOwl:id>GAZ:00387399</oboInOwl:id>
        <rdfs:label>KwaZulu-Natal National Botanical Garden</rdfs:label>
    </owl:NamedIndividual>
    


    <!-- http://purl.obolibrary.org/obo/GAZ_00387400 -->

    <owl:NamedIndividual rdf:about="http://purl.obolibrary.org/obo/GAZ_00387400">
        <obo:RO_0001025 rdf:resource="http://purl.obolibrary.org/obo/GAZ_00076057"/>
        <obo:IAO_0000115>A populated place.</obo:IAO_0000115>
        <oboInOwl:hasOBONamespace>GAZ</oboInOwl:hasOBONamespace>
        <oboInOwl:id>GAZ:00387400</oboInOwl:id>
        <rdfs:label>Daantjie</rdfs:label>
    </owl:NamedIndividual>
    


    <!-- http://purl.obolibrary.org/obo/GAZ_00387401 -->

    <owl:NamedIndividual rdf:about="http://purl.obolibrary.org/obo/GAZ_00387401">
        <obo:RO_0001025 rdf:resource="http://purl.obolibrary.org/obo/GAZ_00076057"/>
        <obo:IAO_0000115>A populated place.</obo:IAO_0000115>
        <oboInOwl:hasOBONamespace>GAZ</oboInOwl:hasOBONamespace>
        <oboInOwl:id>GAZ:00387401</oboInOwl:id>
        <rdfs:label>Kaapsehoop</rdfs:label>
    </owl:NamedIndividual>
    


    <!-- http://purl.obolibrary.org/obo/GAZ_00387402 -->

    <owl:NamedIndividual rdf:about="http://purl.obolibrary.org/obo/GAZ_00387402">
        <obo:RO_0001025 rdf:resource="http://purl.obolibrary.org/obo/GAZ_00076057"/>
        <obo:IAO_0000115>A populated place.</obo:IAO_0000115>
        <oboInOwl:hasOBONamespace>GAZ</oboInOwl:hasOBONamespace>
        <oboInOwl:id>GAZ:00387402</oboInOwl:id>
        <rdfs:label>Kabowkeni</rdfs:label>
    </owl:NamedIndividual>
    


    <!-- http://purl.obolibrary.org/obo/GAZ_00387403 -->

    <owl:NamedIndividual rdf:about="http://purl.obolibrary.org/obo/GAZ_00387403">
        <obo:RO_0001025 rdf:resource="http://purl.obolibrary.org/obo/GAZ_00076057"/>
        <obo:IAO_0000115>A populated place.</obo:IAO_0000115>
        <oboInOwl:hasOBONamespace>GAZ</oboInOwl:hasOBONamespace>
        <oboInOwl:id>GAZ:00387403</oboInOwl:id>
        <rdfs:label>Kanyamazane</rdfs:label>
    </owl:NamedIndividual>
    


    <!-- http://purl.obolibrary.org/obo/GAZ_00387404 -->

    <owl:NamedIndividual rdf:about="http://purl.obolibrary.org/obo/GAZ_00387404">
        <obo:RO_0001025 rdf:resource="http://purl.obolibrary.org/obo/GAZ_00076057"/>
        <obo:IAO_0000115>A populated place.</obo:IAO_0000115>
        <oboInOwl:hasOBONamespace>GAZ</oboInOwl:hasOBONamespace>
        <oboInOwl:id>GAZ:00387404</oboInOwl:id>
        <rdfs:label>Hazyview</rdfs:label>
    </owl:NamedIndividual>
    


    <!-- http://purl.obolibrary.org/obo/GAZ_00387405 -->

    <owl:NamedIndividual rdf:about="http://purl.obolibrary.org/obo/GAZ_00387405">
        <obo:RO_0001025 rdf:resource="http://purl.obolibrary.org/obo/GAZ_00076057"/>
        <obo:IAO_0000115>A populated place.</obo:IAO_0000115>
        <oboInOwl:hasOBONamespace>GAZ</oboInOwl:hasOBONamespace>
        <oboInOwl:id>GAZ:00387405</oboInOwl:id>
        <rdfs:label>Matsulu</rdfs:label>
    </owl:NamedIndividual>
    


    <!-- http://purl.obolibrary.org/obo/GAZ_00387406 -->

    <owl:NamedIndividual rdf:about="http://purl.obolibrary.org/obo/GAZ_00387406">
        <obo:RO_0001025 rdf:resource="http://purl.obolibrary.org/obo/GAZ_00076057"/>
        <obo:IAO_0000115>A populated place.</obo:IAO_0000115>
        <oboInOwl:hasOBONamespace>GAZ</oboInOwl:hasOBONamespace>
        <oboInOwl:id>GAZ:00387406</oboInOwl:id>
        <rdfs:label>Mpakeni</rdfs:label>
    </owl:NamedIndividual>
    


    <!-- http://purl.obolibrary.org/obo/GAZ_00387407 -->

    <owl:NamedIndividual rdf:about="http://purl.obolibrary.org/obo/GAZ_00387407">
        <obo:RO_0001025 rdf:resource="http://purl.obolibrary.org/obo/GAZ_00076057"/>
        <obo:IAO_0000115>A populated place.</obo:IAO_0000115>
        <oboInOwl:hasOBONamespace>GAZ</oboInOwl:hasOBONamespace>
        <oboInOwl:id>GAZ:00387407</oboInOwl:id>
        <rdfs:label>Msogwaba</rdfs:label>
    </owl:NamedIndividual>
    


    <!-- http://purl.obolibrary.org/obo/GAZ_00387408 -->

    <owl:NamedIndividual rdf:about="http://purl.obolibrary.org/obo/GAZ_00387408">
        <obo:RO_0001025 rdf:resource="http://purl.obolibrary.org/obo/GAZ_00076057"/>
        <obo:IAO_0000115>A populated place.</obo:IAO_0000115>
        <oboInOwl:hasOBONamespace>GAZ</oboInOwl:hasOBONamespace>
        <oboInOwl:id>GAZ:00387408</oboInOwl:id>
        <rdfs:label>Ngodwana</rdfs:label>
    </owl:NamedIndividual>
    


    <!-- http://purl.obolibrary.org/obo/GAZ_00387409 -->

    <owl:NamedIndividual rdf:about="http://purl.obolibrary.org/obo/GAZ_00387409">
        <obo:RO_0001025 rdf:resource="http://purl.obolibrary.org/obo/GAZ_00076057"/>
        <obo:IAO_0000115>A populated place.</obo:IAO_0000115>
        <oboInOwl:hasOBONamespace>GAZ</oboInOwl:hasOBONamespace>
        <oboInOwl:id>GAZ:00387409</oboInOwl:id>
        <rdfs:label>Nsikazi</rdfs:label>
    </owl:NamedIndividual>
    


    <!-- http://purl.obolibrary.org/obo/GAZ_00387410 -->

    <owl:NamedIndividual rdf:about="http://purl.obolibrary.org/obo/GAZ_00387410">
        <obo:RO_0001025 rdf:resource="http://purl.obolibrary.org/obo/GAZ_00076057"/>
        <obo:IAO_0000115>A populated place.</obo:IAO_0000115>
        <oboInOwl:hasOBONamespace>GAZ</oboInOwl:hasOBONamespace>
        <oboInOwl:id>GAZ:00387410</oboInOwl:id>
        <rdfs:label>Rocky&apos;s Drift</rdfs:label>
    </owl:NamedIndividual>
    


    <!-- http://purl.obolibrary.org/obo/GAZ_00387411 -->

    <owl:NamedIndividual rdf:about="http://purl.obolibrary.org/obo/GAZ_00387411">
        <obo:RO_0001025 rdf:resource="http://purl.obolibrary.org/obo/GAZ_00076057"/>
        <obo:IAO_0000115>A populated place.</obo:IAO_0000115>
        <oboInOwl:hasOBONamespace>GAZ</oboInOwl:hasOBONamespace>
        <oboInOwl:id>GAZ:00387411</oboInOwl:id>
        <rdfs:label>Tekwane</rdfs:label>
    </owl:NamedIndividual>
    


    <!-- http://purl.obolibrary.org/obo/GAZ_00387412 -->

    <owl:NamedIndividual rdf:about="http://purl.obolibrary.org/obo/GAZ_00387412">
        <obo:RO_0001025 rdf:resource="http://purl.obolibrary.org/obo/GAZ_00076057"/>
        <obo:IAO_0000115>A populated place.</obo:IAO_0000115>
        <oboInOwl:hasOBONamespace>GAZ</oboInOwl:hasOBONamespace>
        <oboInOwl:id>GAZ:00387412</oboInOwl:id>
        <rdfs:label>White River</rdfs:label>
    </owl:NamedIndividual>
    


    <!-- http://purl.obolibrary.org/obo/GAZ_00387413 -->

    <owl:NamedIndividual rdf:about="http://purl.obolibrary.org/obo/GAZ_00387413">
        <obo:RO_0001025 rdf:resource="http://purl.obolibrary.org/obo/GAZ_00005307"/>
        <obo:IAO_0000115>A botanical garden.</obo:IAO_0000115>
        <oboInOwl:hasOBONamespace>GAZ</oboInOwl:hasOBONamespace>
        <oboInOwl:id>GAZ:00387413</oboInOwl:id>
        <rdfs:label>Lowveld National Botanical Garden</rdfs:label>
    </owl:NamedIndividual>
    


    <!-- http://purl.obolibrary.org/obo/GAZ_22223594 -->

    <owl:NamedIndividual rdf:about="http://purl.obolibrary.org/obo/GAZ_22223594">
        <obo:RO_0001025 rdf:resource="http://purl.obolibrary.org/obo/GAZ_00032872"/>
        <obo:IAO_0000115>A District Management Area in Namakwa District Municipality.</obo:IAO_0000115>
        <oboInOwl:hasOBONamespace>GAZ</oboInOwl:hasOBONamespace>
        <oboInOwl:id>GAZ:22223594</oboInOwl:id>
        <rdfs:label>Namaqualand District Management Area</rdfs:label>
    </owl:NamedIndividual>
    


    <!-- http://purl.obolibrary.org/obo/GAZ_22223595 -->

    <owl:NamedIndividual rdf:about="http://purl.obolibrary.org/obo/GAZ_22223595">
        <obo:RO_0001025 rdf:resource="http://purl.obolibrary.org/obo/GAZ_22223594"/>
        <oboInOwl:hasOBONamespace>GAZ</oboInOwl:hasOBONamespace>
        <oboInOwl:id>GAZ:22223595</oboInOwl:id>
        <rdfs:label>Steinkopf</rdfs:label>
    </owl:NamedIndividual>
    


    <!-- http://purl.obolibrary.org/obo/GAZ_22223611 -->

    <owl:NamedIndividual rdf:about="http://purl.obolibrary.org/obo/GAZ_22223611">
        <obo:RO_0001025 rdf:resource="http://purl.obolibrary.org/obo/GAZ_00076005"/>
    </owl:NamedIndividual>
    


    <!-- http://purl.obolibrary.org/obo/GAZ_22223612 -->

    <owl:NamedIndividual rdf:about="http://purl.obolibrary.org/obo/GAZ_22223612">
        <obo:RO_0001025 rdf:resource="http://purl.obolibrary.org/obo/GAZ_00076005"/>
    </owl:NamedIndividual>
    


    <!-- http://purl.obolibrary.org/obo/GAZ_22223613 -->

    <owl:NamedIndividual rdf:about="http://purl.obolibrary.org/obo/GAZ_22223613">
        <obo:RO_0001025 rdf:resource="http://purl.obolibrary.org/obo/GAZ_00076005"/>
    </owl:NamedIndividual>
    


    <!-- http://purl.obolibrary.org/obo/GAZ_22223614 -->

    <owl:NamedIndividual rdf:about="http://purl.obolibrary.org/obo/GAZ_22223614">
        <obo:RO_0001025 rdf:resource="http://purl.obolibrary.org/obo/GAZ_00076005"/>
    </owl:NamedIndividual>
    


    <!-- http://purl.obolibrary.org/obo/GAZ_22223615 -->

    <owl:NamedIndividual rdf:about="http://purl.obolibrary.org/obo/GAZ_22223615">
        <obo:RO_0001025 rdf:resource="http://purl.obolibrary.org/obo/GAZ_00076005"/>
    </owl:NamedIndividual>
    


    <!-- http://purl.obolibrary.org/obo/GAZ_22223616 -->

    <owl:NamedIndividual rdf:about="http://purl.obolibrary.org/obo/GAZ_22223616">
        <obo:RO_0001025 rdf:resource="http://purl.obolibrary.org/obo/GAZ_00076005"/>
    </owl:NamedIndividual>
    


    <!-- http://purl.obolibrary.org/obo/GAZ_22223617 -->

    <owl:NamedIndividual rdf:about="http://purl.obolibrary.org/obo/GAZ_22223617">
        <obo:RO_0001025 rdf:resource="http://purl.obolibrary.org/obo/GAZ_00076005"/>
    </owl:NamedIndividual>
    


    <!-- http://purl.obolibrary.org/obo/GAZ_22223618 -->

    <owl:NamedIndividual rdf:about="http://purl.obolibrary.org/obo/GAZ_22223618">
        <obo:RO_0001025 rdf:resource="http://purl.obolibrary.org/obo/GAZ_00076005"/>
    </owl:NamedIndividual>
    


    <!-- http://purl.obolibrary.org/obo/GAZ_22223619 -->

    <owl:NamedIndividual rdf:about="http://purl.obolibrary.org/obo/GAZ_22223619">
        <obo:RO_0001025 rdf:resource="http://purl.obolibrary.org/obo/GAZ_00076005"/>
    </owl:NamedIndividual>
    


    <!-- http://purl.obolibrary.org/obo/GAZ_22223620 -->

    <owl:NamedIndividual rdf:about="http://purl.obolibrary.org/obo/GAZ_22223620">
        <obo:RO_0001025 rdf:resource="http://purl.obolibrary.org/obo/GAZ_00076006"/>
    </owl:NamedIndividual>
    


    <!-- http://purl.obolibrary.org/obo/GAZ_22223621 -->

    <owl:NamedIndividual rdf:about="http://purl.obolibrary.org/obo/GAZ_22223621">
        <obo:RO_0001025 rdf:resource="http://purl.obolibrary.org/obo/GAZ_00076006"/>
    </owl:NamedIndividual>
    


    <!-- http://purl.obolibrary.org/obo/GAZ_22223622 -->

    <owl:NamedIndividual rdf:about="http://purl.obolibrary.org/obo/GAZ_22223622">
        <obo:RO_0001025 rdf:resource="http://purl.obolibrary.org/obo/GAZ_00076006"/>
    </owl:NamedIndividual>
    


    <!-- http://purl.obolibrary.org/obo/GAZ_22223623 -->

    <owl:NamedIndividual rdf:about="http://purl.obolibrary.org/obo/GAZ_22223623">
        <obo:RO_0001025 rdf:resource="http://purl.obolibrary.org/obo/GAZ_00076006"/>
    </owl:NamedIndividual>
    


    <!-- http://purl.obolibrary.org/obo/GAZ_22223624 -->

    <owl:NamedIndividual rdf:about="http://purl.obolibrary.org/obo/GAZ_22223624">
        <obo:RO_0001025 rdf:resource="http://purl.obolibrary.org/obo/GAZ_00076006"/>
    </owl:NamedIndividual>
    


    <!-- http://purl.obolibrary.org/obo/GAZ_22223625 -->

    <owl:NamedIndividual rdf:about="http://purl.obolibrary.org/obo/GAZ_22223625">
        <obo:RO_0001025 rdf:resource="http://purl.obolibrary.org/obo/GAZ_00076007"/>
    </owl:NamedIndividual>
    


    <!-- http://purl.obolibrary.org/obo/GAZ_22223626 -->

    <owl:NamedIndividual rdf:about="http://purl.obolibrary.org/obo/GAZ_22223626">
        <obo:RO_0001025 rdf:resource="http://purl.obolibrary.org/obo/GAZ_00076007"/>
    </owl:NamedIndividual>
    


    <!-- http://purl.obolibrary.org/obo/GAZ_22223627 -->

    <owl:NamedIndividual rdf:about="http://purl.obolibrary.org/obo/GAZ_22223627">
        <obo:RO_0001025 rdf:resource="http://purl.obolibrary.org/obo/GAZ_00076007"/>
    </owl:NamedIndividual>
    


    <!-- http://purl.obolibrary.org/obo/GAZ_22223628 -->

    <owl:NamedIndividual rdf:about="http://purl.obolibrary.org/obo/GAZ_22223628">
        <obo:RO_0001025 rdf:resource="http://purl.obolibrary.org/obo/GAZ_00032878"/>
    </owl:NamedIndividual>
    


    <!-- http://purl.obolibrary.org/obo/GAZ_22223629 -->

    <owl:NamedIndividual rdf:about="http://purl.obolibrary.org/obo/GAZ_22223629">
        <obo:RO_0001025 rdf:resource="http://purl.obolibrary.org/obo/GAZ_00032873"/>
        <obo:IAO_0000115>A local municipality in Siyanda District Municipality.</obo:IAO_0000115>
        <oboInOwl:hasOBONamespace>GAZ</oboInOwl:hasOBONamespace>
        <oboInOwl:id>GAZ:22223629</oboInOwl:id>
        <rdfs:label>Kgatelopele Local Municipality</rdfs:label>
    </owl:NamedIndividual>
    


    <!-- http://purl.obolibrary.org/obo/GAZ_22223630 -->

    <owl:NamedIndividual rdf:about="http://purl.obolibrary.org/obo/GAZ_22223630">
        <obo:RO_0001025 rdf:resource="http://purl.obolibrary.org/obo/GAZ_22223629"/>
    </owl:NamedIndividual>
    


    <!-- http://purl.obolibrary.org/obo/GAZ_22224454 -->

    <owl:NamedIndividual rdf:about="http://purl.obolibrary.org/obo/GAZ_22224454">
        <obo:RO_0001025 rdf:resource="http://purl.obolibrary.org/obo/GAZ_00032886"/>
        <obo:IAO_0000115>A local municipality in the Nkangala District Minicipality of in the Mpumalanga Province.</obo:IAO_0000115>
        <oboInOwl:hasOBONamespace>GAZ</oboInOwl:hasOBONamespace>
        <oboInOwl:id>GAZ:22224454</oboInOwl:id>
        <rdfs:label>Middelburg Local Municipality</rdfs:label>
    </owl:NamedIndividual>
    


    <!-- http://purl.obolibrary.org/obo/GAZ_22224455 -->

    <owl:NamedIndividual rdf:about="http://purl.obolibrary.org/obo/GAZ_22224455">
        <obo:RO_0001025 rdf:resource="http://purl.obolibrary.org/obo/GAZ_22224454"/>
    </owl:NamedIndividual>
    


    <!-- 
    ///////////////////////////////////////////////////////////////////////////////////////
    //
    // Annotations
    //
    ///////////////////////////////////////////////////////////////////////////////////////
     -->

    <rdf:Description rdf:about="http://purl.obolibrary.org/obo/GAZ_00002810">
        <rdfs:label>Province (Republic of South Africa)</rdfs:label>
        <oboInOwl:hasOBONamespace>GAZ</oboInOwl:hasOBONamespace>
        <oboInOwl:id>GAZ:00002810</oboInOwl:id>
    </rdf:Description>
    <rdf:Description rdf:about="http://purl.obolibrary.org/obo/GAZ_00002811">
        <rdfs:label>North West Province</rdfs:label>
        <oboInOwl:id>GAZ:00002811</oboInOwl:id>
        <oboInOwl:hasOBONamespace>GAZ</oboInOwl:hasOBONamespace>
        <obo:IAO_0000115>A province of South Africa. Its capital is Mafikeng. It created in 1994, and includes parts of the former Transvaal province and Cape Province, as well as most of the former Bantustan of Bophuthatswana.</obo:IAO_0000115>
    </rdf:Description>
    <rdf:Description rdf:about="http://purl.obolibrary.org/obo/GAZ_00002812">
        <obo:IAO_0000115>A province of South Africa. Prior to 1994 the territory now known as KwaZulu-Natal was made up of the province of Natal and all pieces of territory that made up the homeland of KwaZulu.</obo:IAO_0000115>
        <rdfs:label>KwaZulu-Natal Province</rdfs:label>
        <oboInOwl:id>GAZ:00002812</oboInOwl:id>
        <oboInOwl:hasOBONamespace>GAZ</oboInOwl:hasOBONamespace>
    </rdf:Description>
    <rdf:Description rdf:about="http://purl.obolibrary.org/obo/GAZ_00002813">
        <obo:IAO_0000115>A province of South Africa. The current borders date from 1994 when the Bantustans were abolished and included into the provinces of South Africa.</obo:IAO_0000115>
        <oboInOwl:id>GAZ:00002813</oboInOwl:id>
        <oboInOwl:hasOBONamespace>GAZ</oboInOwl:hasOBONamespace>
        <rdfs:label>Free State Province</rdfs:label>
    </rdf:Description>
    <rdf:Description rdf:about="http://purl.obolibrary.org/obo/GAZ_00002814">
        <oboInOwl:hasOBONamespace>GAZ</oboInOwl:hasOBONamespace>
        <obo:IAO_0000115>The northernmost province of South Africa. The capital is Polokwane, former called Pietersburg. The province was formed from the northern region of the Transvaal province in 1994, and initially named Northern Transvaal. The following year, it was renamed Northern Province, which remained the name until 2003-06-11, when the name of the province was formally changed to the name of its most important river.</obo:IAO_0000115>
        <rdfs:label>Limpopo Province</rdfs:label>
        <oboInOwl:id>GAZ:00002814</oboInOwl:id>
    </rdf:Description>
    <rdf:Description rdf:about="http://purl.obolibrary.org/obo/GAZ_00002815">
        <oboInOwl:hasOBONamespace>GAZ</oboInOwl:hasOBONamespace>
        <rdfs:label>Gauteng Province</rdfs:label>
        <obo:IAO_0000115>A province of South Africa. It was formed from part of the old Transvaal province.</obo:IAO_0000115>
        <oboInOwl:id>GAZ:00002815</oboInOwl:id>
    </rdf:Description>
    <rdf:Description rdf:about="http://purl.obolibrary.org/obo/GAZ_00002816">
        <oboInOwl:hasOBONamespace>GAZ</oboInOwl:hasOBONamespace>
        <rdfs:label>Mpumalanga Province</rdfs:label>
        <oboInOwl:id>GAZ:00002816</oboInOwl:id>
        <obo:IAO_0000115>A province in South Africa. Mpumalanga lies in eastern South Africa, north of KwaZulu-Natal and bordering Swaziland and Mozambique. In the north it borders on Limpopo, to the west Gauteng, to the southwest the Free State and to the south KwaZulu-Natal. The capital is Nelspruit.</obo:IAO_0000115>
    </rdf:Description>
    <rdf:Description rdf:about="http://purl.obolibrary.org/obo/GAZ_00002817">
        <rdfs:label>Western Cape Province</rdfs:label>
        <oboInOwl:hasOBONamespace>GAZ</oboInOwl:hasOBONamespace>
        <oboInOwl:id>GAZ:00002817</oboInOwl:id>
        <obo:IAO_0000115>A province in the south west of South Africa. The capital is Cape Town. Prior to 1994, the region that now forms the Western Cape was part of the huge (and now defunct) Cape Province. Prior to the formation of the Union of South Africa in 1910, it was called the Cape Colony.</obo:IAO_0000115>
    </rdf:Description>
    <rdf:Description rdf:about="http://purl.obolibrary.org/obo/GAZ_00002818">
        <oboInOwl:hasOBONamespace>GAZ</oboInOwl:hasOBONamespace>
        <oboInOwl:id>GAZ:00002818</oboInOwl:id>
        <obo:IAO_0000115>A large, sparsely populated province of South Africa, created in 1994 when the Cape Province was split up. Its capital is Kimberley. It includes the Kalahari Gemsbok National Park, which is part of a trans-frontier park with Botswana.</obo:IAO_0000115>
        <rdfs:label>Northern Cape Province</rdfs:label>
    </rdf:Description>
    <rdf:Description rdf:about="http://purl.obolibrary.org/obo/GAZ_00002819">
        <rdfs:label>Eastern Cape Province</rdfs:label>
        <oboInOwl:hasOBONamespace>GAZ</oboInOwl:hasOBONamespace>
        <oboInOwl:id>GAZ:00002819</oboInOwl:id>
        <obo:IAO_0000115>A province of South Africa. Its capital is Bhisho. It was formed in 1994 out of the &quot;independent&quot; homelands of Transkei and Ciskei, as well as the eastern portion of the Cape Province.</obo:IAO_0000115>
    </rdf:Description>
    <rdf:Description rdf:about="http://purl.obolibrary.org/obo/GAZ_00003034">
        <oboInOwl:id>GAZ:00003034</oboInOwl:id>
        <oboInOwl:hasOBONamespace>GAZ</oboInOwl:hasOBONamespace>
        <rdfs:label>populated place, Republic of South Africa</rdfs:label>
    </rdf:Description>
    <rdf:Description rdf:about="http://purl.obolibrary.org/obo/GAZ_00003035">
        <oboInOwl:hasOBONamespace>GAZ</oboInOwl:hasOBONamespace>
        <oboInOwl:id>GAZ:00003035</oboInOwl:id>
        <rdfs:label>Johannesburg</rdfs:label>
    </rdf:Description>
    <rdf:Description rdf:about="http://purl.obolibrary.org/obo/GAZ_00003725">
        <obo:IAO_0000115>A small town in Mpumalanga Province, South Africa.</obo:IAO_0000115>
        <rdfs:label>Belfast</rdfs:label>
        <oboInOwl:hasOBONamespace>GAZ</oboInOwl:hasOBONamespace>
        <oboInOwl:id>GAZ:00003725</oboInOwl:id>
    </rdf:Description>
    <rdf:Description rdf:about="http://purl.obolibrary.org/obo/GAZ_00003726">
        <obo:IAO_0000115>A populated place. A town situated on a tributary of the Mkhomazi River in the midlands of KwaZulu-Natal, South Africa.</obo:IAO_0000115>
        <oboInOwl:id>GAZ:00003726</oboInOwl:id>
        <oboInOwl:hasOBONamespace>GAZ</oboInOwl:hasOBONamespace>
        <rdfs:label>Ixopo</rdfs:label>
    </rdf:Description>
    <rdf:Description rdf:about="http://purl.obolibrary.org/obo/GAZ_00005305">
        <oboInOwl:id>GAZ:00005305</oboInOwl:id>
        <oboInOwl:hasOBONamespace>GAZ</oboInOwl:hasOBONamespace>
        <rdfs:label>Knysna</rdfs:label>
        <obo:IAO_0000115>A populated place. A town in the Western Cape Province of South Africa.</obo:IAO_0000115>
    </rdf:Description>
    <rdf:Description rdf:about="http://purl.obolibrary.org/obo/GAZ_00005306">
        <obo:IAO_0000115>A populated place. A city in the Western Cape Province of South Africa, forming part of the metropolitan municipality of the City of Cape Town.</obo:IAO_0000115>
        <oboInOwl:id>GAZ:00005306</oboInOwl:id>
        <rdfs:label>Cape Town</rdfs:label>
        <oboInOwl:hasOBONamespace>GAZ</oboInOwl:hasOBONamespace>
    </rdf:Description>
    <rdf:Description rdf:about="http://purl.obolibrary.org/obo/GAZ_00005310">
        <oboInOwl:id>GAZ:00005310</oboInOwl:id>
        <obo:IAO_0000115>A small mixed farming town in the Free State province of South Africa. Winburg is situated midway between the Orange River and the Vaal River, adjacent to the N1 National Road, which links Cape Town to Johannesburg. The nearest city, Bloemfontein, is 120 km away.</obo:IAO_0000115>
        <rdfs:label>Winburg</rdfs:label>
        <oboInOwl:hasOBONamespace>GAZ</oboInOwl:hasOBONamespace>
    </rdf:Description>
    <rdf:Description rdf:about="http://purl.obolibrary.org/obo/GAZ_00005311">
        <oboInOwl:id>GAZ:00005311</oboInOwl:id>
        <rdfs:label>Pretoria</rdfs:label>
        <obo:IAO_0000115>A city located in the northern part of Gauteng Province, South Africa.</obo:IAO_0000115>
        <oboInOwl:hasOBONamespace>GAZ</oboInOwl:hasOBONamespace>
    </rdf:Description>
    <rdf:Description rdf:about="http://purl.obolibrary.org/obo/GAZ_00005314">
        <rdfs:label>Stellenbosch</rdfs:label>
        <oboInOwl:hasOBONamespace>GAZ</oboInOwl:hasOBONamespace>
        <oboInOwl:id>GAZ:00005314</oboInOwl:id>
        <obo:IAO_0000115>A populated place. A town in the Western Cape province of South Africa.</obo:IAO_0000115>
    </rdf:Description>
    <rdf:Description rdf:about="http://purl.obolibrary.org/obo/GAZ_00005316">
        <obo:IAO_0000115>A farming town situated 32 km North of the Loskop Dam in the Sekhukhune District of Limpopo.</obo:IAO_0000115>
        <oboInOwl:hasOBONamespace>GAZ</oboInOwl:hasOBONamespace>
        <rdfs:label>Groblersdal</rdfs:label>
        <oboInOwl:id>GAZ:00005316</oboInOwl:id>
    </rdf:Description>
    <rdf:Description rdf:about="http://purl.obolibrary.org/obo/GAZ_00008041">
        <oboInOwl:hasOBONamespace>GAZ</oboInOwl:hasOBONamespace>
        <rdfs:label>Pietermaritzburg</rdfs:label>
        <oboInOwl:id>GAZ:00008041</oboInOwl:id>
        <obo:IAO_0000115>The capital and second largest city of the province of KwaZulu-Natal in South Africa.</obo:IAO_0000115>
    </rdf:Description>
    <rdf:Description rdf:about="http://purl.obolibrary.org/obo/GAZ_00010007">
        <rdfs:label>Durban</rdfs:label>
        <obo:IAO_0000115>The third most populous city in South Africa, forming part of the eThekwini metropolitan municipality.</obo:IAO_0000115>
        <oboInOwl:hasOBONamespace>GAZ</oboInOwl:hasOBONamespace>
        <oboInOwl:id>GAZ:00010007</oboInOwl:id>
    </rdf:Description>
    <rdf:Description rdf:about="http://purl.obolibrary.org/obo/GAZ_00010008">
        <oboInOwl:hasOBONamespace>GAZ</oboInOwl:hasOBONamespace>
        <rdfs:label>Derby</rdfs:label>
        <obo:IAO_0000115>A small town situated in North West Province of South Africa.</obo:IAO_0000115>
        <oboInOwl:id>GAZ:00010008</oboInOwl:id>
    </rdf:Description>
    <rdf:Description rdf:about="http://purl.obolibrary.org/obo/GAZ_00052064">
        <oboInOwl:id>GAZ:00052064</oboInOwl:id>
        <oboInOwl:hasOBONamespace>GAZ</oboInOwl:hasOBONamespace>
        <obo:IAO_0000115>A gold-mining town in western Gauteng, South Africa.</obo:IAO_0000115>
        <rdfs:label>Carletonville</rdfs:label>
    </rdf:Description>
    <rdf:Description rdf:about="http://purl.obolibrary.org/obo/GAZ_00052087">
        <obo:IAO_0000115>A populated place. A city in South Africa, situated in the Eastern Cape Province, 770 km east of Cape Town.</obo:IAO_0000115>
        <rdfs:label>Port Elizabeth</rdfs:label>
        <oboInOwl:hasOBONamespace>GAZ</oboInOwl:hasOBONamespace>
        <oboInOwl:id>GAZ:00052087</oboInOwl:id>
    </rdf:Description>
    <rdf:Description rdf:about="http://purl.obolibrary.org/obo/GAZ_00052090">
        <rdfs:label>Welkom</rdfs:label>
        <obo:IAO_0000115>A city that is 60 km northeast of Bloemfontein, the provincial capital. The town is the hub of the Free State gold fields, serving several gold and uranium mines.</obo:IAO_0000115>
        <oboInOwl:hasOBONamespace>GAZ</oboInOwl:hasOBONamespace>
        <oboInOwl:id>GAZ:00052090</oboInOwl:id>
    </rdf:Description>
    <rdf:Description rdf:about="http://purl.obolibrary.org/obo/GAZ_00239919">
        <obo:IAO_0000115>A protected area.</obo:IAO_0000115>
        <oboInOwl:hasOBONamespace>GAZ</oboInOwl:hasOBONamespace>
        <oboInOwl:id>GAZ:00239919</oboInOwl:id>
        <rdfs:label>Boskop Dam Nature Reserve</rdfs:label>
    </rdf:Description>
    <rdf:Description rdf:about="http://purl.obolibrary.org/obo/GAZ_00281455">
        <oboInOwl:hasOBONamespace>GAZ</oboInOwl:hasOBONamespace>
        <rdfs:label>Waterval Boven</rdfs:label>
        <obo:IAO_0000115>A populated place.</obo:IAO_0000115>
        <oboInOwl:id>GAZ:00281455</oboInOwl:id>
    </rdf:Description>
    <rdf:Description rdf:about="http://purl.obolibrary.org/obo/GAZ_00281473">
        <obo:IAO_0000115>A populated place.</obo:IAO_0000115>
        <rdfs:label>Lindley</rdfs:label>
        <oboInOwl:hasOBONamespace>GAZ</oboInOwl:hasOBONamespace>
        <oboInOwl:id>GAZ:00281473</oboInOwl:id>
    </rdf:Description>
    <rdf:Description rdf:about="http://purl.obolibrary.org/obo/GAZ_22223611">
        <oboInOwl:id>GAZ:22223611</oboInOwl:id>
        <oboInOwl:hasOBONamespace>GAZ</oboInOwl:hasOBONamespace>
        <rdfs:label>Fauresmith</rdfs:label>
    </rdf:Description>
    <rdf:Description rdf:about="http://purl.obolibrary.org/obo/GAZ_22223612">
        <oboInOwl:id>GAZ:22223612</oboInOwl:id>
        <oboInOwl:hasOBONamespace>GAZ</oboInOwl:hasOBONamespace>
        <rdfs:label>Jagersfontein</rdfs:label>
    </rdf:Description>
    <rdf:Description rdf:about="http://purl.obolibrary.org/obo/GAZ_22223613">
        <oboInOwl:id>GAZ:22223613</oboInOwl:id>
        <rdfs:label>Philippolis</rdfs:label>
        <oboInOwl:hasOBONamespace>GAZ</oboInOwl:hasOBONamespace>
    </rdf:Description>
    <rdf:Description rdf:about="http://purl.obolibrary.org/obo/GAZ_22223614">
        <oboInOwl:hasOBONamespace>GAZ</oboInOwl:hasOBONamespace>
        <rdfs:label>Bethulie</rdfs:label>
        <oboInOwl:id>GAZ:22223614</oboInOwl:id>
    </rdf:Description>
    <rdf:Description rdf:about="http://purl.obolibrary.org/obo/GAZ_22223615">
        <oboInOwl:hasOBONamespace>GAZ</oboInOwl:hasOBONamespace>
        <oboInOwl:id>GAZ:22223615</oboInOwl:id>
        <rdfs:label>Gariep Dam</rdfs:label>
    </rdf:Description>
    <rdf:Description rdf:about="http://purl.obolibrary.org/obo/GAZ_22223616">
        <rdfs:label>Edenburg</rdfs:label>
        <oboInOwl:hasOBONamespace>GAZ</oboInOwl:hasOBONamespace>
        <oboInOwl:id>GAZ:22223616</oboInOwl:id>
    </rdf:Description>
    <rdf:Description rdf:about="http://purl.obolibrary.org/obo/GAZ_22223617">
        <rdfs:label>Springfontein</rdfs:label>
        <oboInOwl:id>GAZ:22223617</oboInOwl:id>
        <oboInOwl:hasOBONamespace>GAZ</oboInOwl:hasOBONamespace>
    </rdf:Description>
    <rdf:Description rdf:about="http://purl.obolibrary.org/obo/GAZ_22223618">
        <rdfs:label>Trompsburg</rdfs:label>
        <oboInOwl:hasOBONamespace>GAZ</oboInOwl:hasOBONamespace>
        <oboInOwl:id>GAZ:22223618</oboInOwl:id>
    </rdf:Description>
    <rdf:Description rdf:about="http://purl.obolibrary.org/obo/GAZ_22223619">
        <oboInOwl:id>GAZ:22223619</oboInOwl:id>
        <rdfs:label>Reddersburg</rdfs:label>
        <oboInOwl:hasOBONamespace>GAZ</oboInOwl:hasOBONamespace>
    </rdf:Description>
    <rdf:Description rdf:about="http://purl.obolibrary.org/obo/GAZ_22223620">
        <oboInOwl:id>GAZ:22223620</oboInOwl:id>
        <oboInOwl:hasOBONamespace>GAZ</oboInOwl:hasOBONamespace>
        <rdfs:label>Luckhoff</rdfs:label>
    </rdf:Description>
    <rdf:Description rdf:about="http://purl.obolibrary.org/obo/GAZ_22223621">
        <oboInOwl:id>GAZ:22223621</oboInOwl:id>
        <oboInOwl:hasOBONamespace>GAZ</oboInOwl:hasOBONamespace>
        <rdfs:label>Petrusburg</rdfs:label>
    </rdf:Description>
    <rdf:Description rdf:about="http://purl.obolibrary.org/obo/GAZ_22223622">
        <rdfs:label>Jacobsdal</rdfs:label>
        <oboInOwl:id>GAZ:22223622</oboInOwl:id>
        <oboInOwl:hasOBONamespace>GAZ</oboInOwl:hasOBONamespace>
    </rdf:Description>
    <rdf:Description rdf:about="http://purl.obolibrary.org/obo/GAZ_22223623">
        <oboInOwl:id>GAZ:22223623</oboInOwl:id>
        <rdfs:label>Oppermansgronde</rdfs:label>
        <oboInOwl:hasOBONamespace>GAZ</oboInOwl:hasOBONamespace>
    </rdf:Description>
    <rdf:Description rdf:about="http://purl.obolibrary.org/obo/GAZ_22223624">
        <rdfs:label>Koffiefontein</rdfs:label>
        <oboInOwl:id>GAZ:22223624</oboInOwl:id>
        <oboInOwl:hasOBONamespace>GAZ</oboInOwl:hasOBONamespace>
    </rdf:Description>
    <rdf:Description rdf:about="http://purl.obolibrary.org/obo/GAZ_22223625">
        <rdfs:label>Zastron</rdfs:label>
        <oboInOwl:id>GAZ:22223625</oboInOwl:id>
        <oboInOwl:hasOBONamespace>GAZ</oboInOwl:hasOBONamespace>
    </rdf:Description>
    <rdf:Description rdf:about="http://purl.obolibrary.org/obo/GAZ_22223626">
        <oboInOwl:id>GAZ:22223626</oboInOwl:id>
        <rdfs:label>Rouxville</rdfs:label>
        <oboInOwl:hasOBONamespace>GAZ</oboInOwl:hasOBONamespace>
    </rdf:Description>
    <rdf:Description rdf:about="http://purl.obolibrary.org/obo/GAZ_22223627">
        <rdfs:label>Smithfield</rdfs:label>
        <oboInOwl:id>GAZ:22223627</oboInOwl:id>
        <oboInOwl:hasOBONamespace>GAZ</oboInOwl:hasOBONamespace>
    </rdf:Description>
    <rdf:Description rdf:about="http://purl.obolibrary.org/obo/GAZ_22223628">
        <rdfs:label>Germiston</rdfs:label>
        <obo:IAO_0000115>A populated place. A city in the East Rand of Gauteng in South Africa.</obo:IAO_0000115>
        <oboInOwl:id>GAZ:22223628</oboInOwl:id>
        <oboInOwl:hasOBONamespace>GAZ</oboInOwl:hasOBONamespace>
    </rdf:Description>
    <rdf:Description rdf:about="http://purl.obolibrary.org/obo/GAZ_22223630">
        <rdfs:label>Danielskuil</rdfs:label>
        <oboInOwl:hasOBONamespace>GAZ</oboInOwl:hasOBONamespace>
        <oboInOwl:id>GAZ:22223630</oboInOwl:id>
    </rdf:Description>
    <rdf:Description rdf:about="http://purl.obolibrary.org/obo/GAZ_22224455">
        <rdfs:label>Middelburg</rdfs:label>
        <oboInOwl:id>GAZ:22224455</oboInOwl:id>
        <oboInOwl:hasOBONamespace>GAZ</oboInOwl:hasOBONamespace>
    </rdf:Description>
</rdf:RDF>



<!-- Generated by the OWL API (version 4.5.6) https://github.com/owlcs/owlapi -->

