<?xml version="1.0"?>
<rdf:RDF xmlns="http://purl.obolibrary.org/obo/gaz/subsets/countries/Saudi_Arabia.owl#"
     xml:base="http://purl.obolibrary.org/obo/gaz/subsets/countries/Saudi_Arabia.owl"
     xmlns:obo="http://purl.obolibrary.org/obo/"
     xmlns:owl="http://www.w3.org/2002/07/owl#"
     xmlns:rdf="http://www.w3.org/1999/02/22-rdf-syntax-ns#"
     xmlns:xml="http://www.w3.org/XML/1998/namespace"
     xmlns:xsd="http://www.w3.org/2001/XMLSchema#"
     xmlns:rdfs="http://www.w3.org/2000/01/rdf-schema#"
     xmlns:oboInOwl="http://www.geneontology.org/formats/oboInOwl#">
    <owl:Ontology rdf:about="http://purl.obolibrary.org/obo/gaz/subsets/countries/Saudi_Arabia.owl">
        <owl:imports rdf:resource="http://purl.obolibrary.org/obo/gaz/imports/envo_import.owl"/>
        <owl:imports rdf:resource="http://purl.obolibrary.org/obo/gaz/imports/ro_import.owl"/>
    </owl:Ontology>
    


    <!-- 
    ///////////////////////////////////////////////////////////////////////////////////////
    //
    // Annotation properties
    //
    ///////////////////////////////////////////////////////////////////////////////////////
     -->

    


    <!-- http://purl.obolibrary.org/obo/IAO_0000115 -->

    <owl:AnnotationProperty rdf:about="http://purl.obolibrary.org/obo/IAO_0000115"/>
    


    <!-- http://www.geneontology.org/formats/oboInOwl#hasOBONamespace -->

    <owl:AnnotationProperty rdf:about="http://www.geneontology.org/formats/oboInOwl#hasOBONamespace"/>
    


    <!-- http://www.geneontology.org/formats/oboInOwl#id -->

    <owl:AnnotationProperty rdf:about="http://www.geneontology.org/formats/oboInOwl#id"/>
    


    <!-- 
    ///////////////////////////////////////////////////////////////////////////////////////
    //
    // Object Properties
    //
    ///////////////////////////////////////////////////////////////////////////////////////
     -->

    


    <!-- http://purl.obolibrary.org/obo/RO_0001025 -->

    <owl:ObjectProperty rdf:about="http://purl.obolibrary.org/obo/RO_0001025"/>
    


    <!-- 
    ///////////////////////////////////////////////////////////////////////////////////////
    //
    // Classes
    //
    ///////////////////////////////////////////////////////////////////////////////////////
     -->

    


    <!-- http://purl.obolibrary.org/obo/ENVO_00000009 -->

    <owl:Class rdf:about="http://purl.obolibrary.org/obo/ENVO_00000009"/>
    


    <!-- http://purl.obolibrary.org/obo/ENVO_00000032 -->

    <owl:Class rdf:about="http://purl.obolibrary.org/obo/ENVO_00000032"/>
    


    <!-- http://purl.obolibrary.org/obo/ENVO_00000033 -->

    <owl:Class rdf:about="http://purl.obolibrary.org/obo/ENVO_00000033"/>
    


    <!-- http://purl.obolibrary.org/obo/ENVO_00000167 -->

    <owl:Class rdf:about="http://purl.obolibrary.org/obo/ENVO_00000167"/>
    


    <!-- http://purl.obolibrary.org/obo/ENVO_00000220 -->

    <owl:Class rdf:about="http://purl.obolibrary.org/obo/ENVO_00000220"/>
    


    <!-- http://purl.obolibrary.org/obo/ENVO_00000222 -->

    <owl:Class rdf:about="http://purl.obolibrary.org/obo/ENVO_00000222"/>
    


    <!-- http://purl.obolibrary.org/obo/ENVO_00000475 -->

    <owl:Class rdf:about="http://purl.obolibrary.org/obo/ENVO_00000475"/>
    


    <!-- http://purl.obolibrary.org/obo/ENVO_00000856 -->

    <owl:Class rdf:about="http://purl.obolibrary.org/obo/ENVO_00000856"/>
    


    <!-- http://purl.obolibrary.org/obo/GAZ_00007506 -->

    <owl:Class rdf:about="http://purl.obolibrary.org/obo/GAZ_00007506">
        <rdfs:subClassOf rdf:resource="http://purl.obolibrary.org/obo/GAZ_00007509"/>
    </owl:Class>
    


    <!-- http://purl.obolibrary.org/obo/GAZ_00007507 -->

    <owl:Class rdf:about="http://purl.obolibrary.org/obo/GAZ_00007507">
        <rdfs:subClassOf rdf:resource="http://purl.obolibrary.org/obo/GAZ_00007508"/>
    </owl:Class>
    


    <!-- http://purl.obolibrary.org/obo/GAZ_00007508 -->

    <owl:Class rdf:about="http://purl.obolibrary.org/obo/GAZ_00007508"/>
    


    <!-- http://purl.obolibrary.org/obo/GAZ_00007509 -->

    <owl:Class rdf:about="http://purl.obolibrary.org/obo/GAZ_00007509"/>
    


    <!-- http://purl.obolibrary.org/obo/GAZ_00009519 -->

    <owl:Class rdf:about="http://purl.obolibrary.org/obo/GAZ_00009519"/>
    


    <!-- http://purl.obolibrary.org/obo/GAZ_00010395 -->

    <owl:Class rdf:about="http://purl.obolibrary.org/obo/GAZ_00010395">
        <rdfs:subClassOf rdf:resource="http://purl.obolibrary.org/obo/GAZ_00007509"/>
    </owl:Class>
    


    <!-- http://purl.obolibrary.org/obo/GAZ_00010396 -->

    <owl:Class rdf:about="http://purl.obolibrary.org/obo/GAZ_00010396">
        <rdfs:subClassOf rdf:resource="http://purl.obolibrary.org/obo/GAZ_00007508"/>
    </owl:Class>
    


    <!-- http://purl.obolibrary.org/obo/GAZ_00010397 -->

    <owl:Class rdf:about="http://purl.obolibrary.org/obo/GAZ_00010397">
        <rdfs:subClassOf rdf:resource="http://purl.obolibrary.org/obo/GAZ_00007509"/>
    </owl:Class>
    


    <!-- http://purl.obolibrary.org/obo/GAZ_00010398 -->

    <owl:Class rdf:about="http://purl.obolibrary.org/obo/GAZ_00010398">
        <rdfs:subClassOf rdf:resource="http://purl.obolibrary.org/obo/GAZ_00007509"/>
    </owl:Class>
    


    <!-- http://purl.obolibrary.org/obo/GAZ_00015054 -->

    <owl:Class rdf:about="http://purl.obolibrary.org/obo/GAZ_00015054">
        <rdfs:subClassOf rdf:resource="http://purl.obolibrary.org/obo/GAZ_00007509"/>
    </owl:Class>
    


    <!-- http://purl.obolibrary.org/obo/GAZ_00015055 -->

    <owl:Class rdf:about="http://purl.obolibrary.org/obo/GAZ_00015055">
        <rdfs:subClassOf rdf:resource="http://purl.obolibrary.org/obo/GAZ_00007509"/>
    </owl:Class>
    


    <!-- http://purl.obolibrary.org/obo/GAZ_00015056 -->

    <owl:Class rdf:about="http://purl.obolibrary.org/obo/GAZ_00015056">
        <rdfs:subClassOf rdf:resource="http://purl.obolibrary.org/obo/GAZ_00007509"/>
    </owl:Class>
    


    <!-- http://purl.obolibrary.org/obo/GAZ_00015057 -->

    <owl:Class rdf:about="http://purl.obolibrary.org/obo/GAZ_00015057">
        <rdfs:subClassOf rdf:resource="http://purl.obolibrary.org/obo/GAZ_00007509"/>
    </owl:Class>
    


    <!-- http://purl.obolibrary.org/obo/GAZ_00015058 -->

    <owl:Class rdf:about="http://purl.obolibrary.org/obo/GAZ_00015058">
        <rdfs:subClassOf rdf:resource="http://purl.obolibrary.org/obo/GAZ_00007509"/>
    </owl:Class>
    


    <!-- http://purl.obolibrary.org/obo/GAZ_00015059 -->

    <owl:Class rdf:about="http://purl.obolibrary.org/obo/GAZ_00015059">
        <rdfs:subClassOf rdf:resource="http://purl.obolibrary.org/obo/GAZ_00007509"/>
    </owl:Class>
    


    <!-- http://purl.obolibrary.org/obo/GAZ_00015060 -->

    <owl:Class rdf:about="http://purl.obolibrary.org/obo/GAZ_00015060">
        <rdfs:subClassOf rdf:resource="http://purl.obolibrary.org/obo/GAZ_00007509"/>
    </owl:Class>
    


    <!-- http://purl.obolibrary.org/obo/GAZ_00015061 -->

    <owl:Class rdf:about="http://purl.obolibrary.org/obo/GAZ_00015061">
        <rdfs:subClassOf rdf:resource="http://purl.obolibrary.org/obo/GAZ_00007509"/>
    </owl:Class>
    


    <!-- http://purl.obolibrary.org/obo/GAZ_00015062 -->

    <owl:Class rdf:about="http://purl.obolibrary.org/obo/GAZ_00015062">
        <rdfs:subClassOf rdf:resource="http://purl.obolibrary.org/obo/GAZ_00007509"/>
    </owl:Class>
    


    <!-- http://purl.obolibrary.org/obo/GAZ_02000358 -->

    <owl:Class rdf:about="http://purl.obolibrary.org/obo/GAZ_02000358">
        <rdfs:subClassOf rdf:resource="http://purl.obolibrary.org/obo/GAZ_00009519"/>
    </owl:Class>
    


    <!-- http://purl.obolibrary.org/obo/GAZ_02000359 -->

    <owl:Class rdf:about="http://purl.obolibrary.org/obo/GAZ_02000359">
        <rdfs:subClassOf rdf:resource="http://purl.obolibrary.org/obo/GAZ_00009519"/>
    </owl:Class>
    


    <!-- http://purl.obolibrary.org/obo/GAZ_02000360 -->

    <owl:Class rdf:about="http://purl.obolibrary.org/obo/GAZ_02000360">
        <rdfs:subClassOf rdf:resource="http://purl.obolibrary.org/obo/GAZ_00009519"/>
    </owl:Class>
    


    <!-- http://purl.obolibrary.org/obo/GAZ_02000361 -->

    <owl:Class rdf:about="http://purl.obolibrary.org/obo/GAZ_02000361">
        <rdfs:subClassOf rdf:resource="http://purl.obolibrary.org/obo/GAZ_00009519"/>
    </owl:Class>
    


    <!-- http://purl.obolibrary.org/obo/GAZ_02000362 -->

    <owl:Class rdf:about="http://purl.obolibrary.org/obo/GAZ_02000362">
        <rdfs:subClassOf rdf:resource="http://purl.obolibrary.org/obo/GAZ_00009519"/>
    </owl:Class>
    


    <!-- 
    ///////////////////////////////////////////////////////////////////////////////////////
    //
    // Individuals
    //
    ///////////////////////////////////////////////////////////////////////////////////////
     -->

    


    <!-- http://purl.obolibrary.org/obo/GAZ_00002456 -->

    <owl:NamedIndividual rdf:about="http://purl.obolibrary.org/obo/GAZ_00002456">
        <obo:IAO_0000115>A sea situated between the coasts of Africa and the Arabian Peninsula, are the following: On the North: A line joining the coast of Africa, in Egypt, eastward, along the parallel of 27 Degrees 27 Minutes N, to the southern extremity of Shaker Island (27 Degrees 27 Minutes N - 34 Degrees 02 Minutes 10 Seconds E), and northeastward to Cape Muhammad (27 Degrees 43 Minutes 35 Seconds N - 34 Degrees 15 Minutes E), the southern extremity of the Sinai Peninsula (the common limit with the Gulf of Suez); thence from Cape Muhammad northeastward, along the southern coast of the Sinai Peninsula, to the parallel of 27 Degrees 54 Minutes 50 Seconds N; thence a line joining the southern coast of the Sinai Peninsula eastward, along the parallel of 27 Degrees 54 Minutes 50 Seconds N, to the southwestern extremity of T Degrees r Degrees n Island (27 Degrees 54 Minutes 50 Seconds N - 34 Degrees 33 Minutes E); thence from the southwestern extremity of T Degrees r Degrees n Island northward, through this island, to position 27 Degrees 58 Minutes 10 Seconds N - 34 Degrees 35 Minutes E), on the northeastern coast thereof; and thence a line joining this position northeastward to Cape Al Qa Degrees bah (28 Degrees 01 Minutes 30 Seconds N - 34 Degrees 37 Minutes 15 Seconds E), in Saudi Arabia (the common limit with the Gulf of Aqaba). On the East: From Cape Al Qa Degrees bah, in Saudi Arabia, southeastward, along the coast of the Arabian Peninsula, to Hisn Mur Degrees d (12 Degrees 40 Minutes 20 Seconds N - 43 Degrees 30 Minutes 20 Seconds E), in Southern Yemen. On the South: A line joining Hisn Mur Degrees d, in Southern Yemen, southwestward to Cape Si Ane (12 Degrees 28 Minutes 50 Seconds N - 43 Degrees 19 Minutes 10 Seconds E), in Djibouti (the common limit with the Gulf of Aden). On the West: From Cape Si Ane, in Djibouti, northwestward, along the coast of Africa, to the parallel of 27 Degrees 27 Minutes N, in Egypt.</obo:IAO_0000115>
        <oboInOwl:hasOBONamespace>GAZ</oboInOwl:hasOBONamespace>
        <oboInOwl:id>GAZ:00002456</oboInOwl:id>
        <rdfs:label>Red Sea</rdfs:label>
    </owl:NamedIndividual>
    


    <!-- http://purl.obolibrary.org/obo/GAZ_00004037 -->

    <owl:NamedIndividual rdf:about="http://purl.obolibrary.org/obo/GAZ_00004037">
        <obo:RO_0001025 rdf:resource="http://purl.obolibrary.org/obo/GAZ_00144637"/>
        <obo:IAO_0000115>A small shore island in the Red Sea. It is owned by Egypt and can be found at the northern entrance to Foul Bay.</obo:IAO_0000115>
        <oboInOwl:hasOBONamespace>GAZ</oboInOwl:hasOBONamespace>
        <oboInOwl:id>GAZ:00004037</oboInOwl:id>
        <rdfs:label>Mukawwar Island</rdfs:label>
    </owl:NamedIndividual>
    


    <!-- http://purl.obolibrary.org/obo/GAZ_00005279 -->

    <owl:NamedIndividual rdf:about="http://purl.obolibrary.org/obo/GAZ_00005279">
        <rdf:type rdf:resource="http://purl.obolibrary.org/obo/ENVO_00000009"/>
        <obo:IAO_0000115>A country on the Arabian Peninsula. It is bordered by Jordan on the northwest, Iraq on the north and northeast, Kuwait, Qatar, Bahrain, and the United Arab Emirates on the east, Oman on the southeast, and Yemen on the south. The Persian Gulf lies to the northeast and the Red Sea to its west. Saudi Arabia is divided into 13 provinces or regions (manatiq; singular mintaqah). Each is then divided into Governorates.</obo:IAO_0000115>
        <oboInOwl:hasOBONamespace>GAZ</oboInOwl:hasOBONamespace>
        <oboInOwl:id>GAZ:00005279</oboInOwl:id>
        <rdfs:label>Saudi Arabia</rdfs:label>
    </owl:NamedIndividual>
    


    <!-- http://purl.obolibrary.org/obo/GAZ_00005281 -->

    <owl:NamedIndividual rdf:about="http://purl.obolibrary.org/obo/GAZ_00005281">
        <obo:RO_0001025 rdf:resource="http://purl.obolibrary.org/obo/GAZ_00006936"/>
        <obo:IAO_0000115>A borderless island country in the Persian Gulf. Saudi Arabia lies to the west and is connected to Bahrain by the King Fahd Causeway, and Qatar is to the south across the Gulf of Bahrain. Bahrain is split into five governorates.</obo:IAO_0000115>
        <oboInOwl:hasOBONamespace>GAZ</oboInOwl:hasOBONamespace>
        <oboInOwl:id>GAZ:00005281</oboInOwl:id>
        <rdfs:label>Bahrain</rdfs:label>
    </owl:NamedIndividual>
    


    <!-- http://purl.obolibrary.org/obo/GAZ_00005295 -->

    <owl:NamedIndividual rdf:about="http://purl.obolibrary.org/obo/GAZ_00005295">
        <obo:IAO_0000115>A gulf bounded by the coasts of Oman, United Arab Emirates, Qatar, Saudi Arabia, Kuwait, Irak and Iran. Its southeastern limit with the Gulf of Oman (in the Strait of Hormuz) is the following: A line joining Cape L Degrees mah (25 Degrees 56 Minutes 35 Seconds N - 56 Degrees 27 Minutes 30 Seconds E), in Oman, eastward to Cape Al K Degrees h (25 Degrees 47 Minutes 30 Seconds N - 57 Degrees 18 Minutes E), in Iran.</obo:IAO_0000115>
        <oboInOwl:hasOBONamespace>GAZ</oboInOwl:hasOBONamespace>
        <oboInOwl:id>GAZ:00005295</oboInOwl:id>
        <rdfs:label>Persian Gulf</rdfs:label>
    </owl:NamedIndividual>
    


    <!-- http://purl.obolibrary.org/obo/GAZ_00005876 -->

    <owl:NamedIndividual rdf:about="http://purl.obolibrary.org/obo/GAZ_00005876">
        <rdf:type rdf:resource="http://purl.obolibrary.org/obo/ENVO_00000220"/>
        <obo:RO_0001025 rdf:resource="http://purl.obolibrary.org/obo/GAZ_00053597"/>
        <obo:IAO_0000115>An island group in the Red Sea. Most of them are a part of Yemen, but before 1998-1999 they were claimed by Eritrea as well. They are formed from a series of volcanic vents along a NE-SW trend, and include the Holocene Great Hanish, Little Hanish, and many other small islands and submarine shoals.</obo:IAO_0000115>
        <oboInOwl:hasOBONamespace>GAZ</oboInOwl:hasOBONamespace>
        <oboInOwl:id>GAZ:00005876</oboInOwl:id>
        <rdfs:label>Hanish Islands</rdfs:label>
    </owl:NamedIndividual>
    


    <!-- http://purl.obolibrary.org/obo/GAZ_00005877 -->

    <owl:NamedIndividual rdf:about="http://purl.obolibrary.org/obo/GAZ_00005877">
        <obo:RO_0001025 rdf:resource="http://purl.obolibrary.org/obo/GAZ_00002456"/>
        <obo:IAO_0000115>A &quot;shelf island&quot; located in the shallow waters of the Arabian peninsula&apos;s continental shelf with coral reefs surrounding three sides of the island.</obo:IAO_0000115>
        <oboInOwl:hasOBONamespace>GAZ</oboInOwl:hasOBONamespace>
        <oboInOwl:id>GAZ:00005877</oboInOwl:id>
        <rdfs:label>Kamaran Island</rdfs:label>
    </owl:NamedIndividual>
    


    <!-- http://purl.obolibrary.org/obo/GAZ_00005878 -->

    <owl:NamedIndividual rdf:about="http://purl.obolibrary.org/obo/GAZ_00005878">
        <rdf:type rdf:resource="http://purl.obolibrary.org/obo/ENVO_00000222"/>
        <obo:RO_0001025 rdf:resource="http://purl.obolibrary.org/obo/GAZ_00051269"/>
        <obo:IAO_0000115>A volcanic island located in the Strait of Mandeb at the southern entrance into the Red Sea off the southwestern coast of Yemen.</obo:IAO_0000115>
        <oboInOwl:hasOBONamespace>GAZ</oboInOwl:hasOBONamespace>
        <oboInOwl:id>GAZ:00005878</oboInOwl:id>
        <rdfs:label>Perim</rdfs:label>
    </owl:NamedIndividual>
    


    <!-- http://purl.obolibrary.org/obo/GAZ_00005879 -->

    <owl:NamedIndividual rdf:about="http://purl.obolibrary.org/obo/GAZ_00005879">
        <obo:RO_0001025 rdf:resource="http://purl.obolibrary.org/obo/GAZ_00053597"/>
        <obo:IAO_0000115>An island of Yemen in the Red Sea. It lies the coasts of Yemen and Eritrea near the Bab-el-Mandeb straits, which connect the Red Sea to the Gulf of Aden. Despite its proximity to the African continent, it is considered an island of Asia because it sits on the Asian continental shelf. A shield volcano.</obo:IAO_0000115>
        <oboInOwl:hasOBONamespace>GAZ</oboInOwl:hasOBONamespace>
        <oboInOwl:id>GAZ:00005879</oboInOwl:id>
        <rdfs:label>Zuqar Island</rdfs:label>
    </owl:NamedIndividual>
    


    <!-- http://purl.obolibrary.org/obo/GAZ_00006936 -->

    <owl:NamedIndividual rdf:about="http://purl.obolibrary.org/obo/GAZ_00006936">
        <obo:RO_0001025 rdf:resource="http://purl.obolibrary.org/obo/GAZ_00005295"/>
        <oboInOwl:hasOBONamespace>GAZ</oboInOwl:hasOBONamespace>
        <oboInOwl:id>GAZ:00006936</oboInOwl:id>
        <rdfs:label>Bahrain Archipelago</rdfs:label>
    </owl:NamedIndividual>
    


    <!-- http://purl.obolibrary.org/obo/GAZ_00006937 -->

    <owl:NamedIndividual rdf:about="http://purl.obolibrary.org/obo/GAZ_00006937">
        <obo:RO_0001025 rdf:resource="http://purl.obolibrary.org/obo/GAZ_00006936"/>
        <oboInOwl:hasOBONamespace>GAZ</oboInOwl:hasOBONamespace>
        <oboInOwl:id>GAZ:00006937</oboInOwl:id>
        <rdfs:label>Bahrain Island</rdfs:label>
    </owl:NamedIndividual>
    


    <!-- http://purl.obolibrary.org/obo/GAZ_00006938 -->

    <owl:NamedIndividual rdf:about="http://purl.obolibrary.org/obo/GAZ_00006938">
        <obo:RO_0001025 rdf:resource="http://purl.obolibrary.org/obo/GAZ_00006936"/>
        <oboInOwl:hasOBONamespace>GAZ</oboInOwl:hasOBONamespace>
        <oboInOwl:id>GAZ:00006938</oboInOwl:id>
        <rdfs:label>Al Muharraq</rdfs:label>
    </owl:NamedIndividual>
    


    <!-- http://purl.obolibrary.org/obo/GAZ_00006939 -->

    <owl:NamedIndividual rdf:about="http://purl.obolibrary.org/obo/GAZ_00006939">
        <obo:RO_0001025 rdf:resource="http://purl.obolibrary.org/obo/GAZ_00006936"/>
        <oboInOwl:hasOBONamespace>GAZ</oboInOwl:hasOBONamespace>
        <oboInOwl:id>GAZ:00006939</oboInOwl:id>
        <rdfs:label>Jazirat al Azl</rdfs:label>
    </owl:NamedIndividual>
    


    <!-- http://purl.obolibrary.org/obo/GAZ_00006940 -->

    <owl:NamedIndividual rdf:about="http://purl.obolibrary.org/obo/GAZ_00006940">
        <obo:RO_0001025 rdf:resource="http://purl.obolibrary.org/obo/GAZ_00006936"/>
        <oboInOwl:hasOBONamespace>GAZ</oboInOwl:hasOBONamespace>
        <oboInOwl:id>GAZ:00006940</oboInOwl:id>
        <rdfs:label>Sitrah</rdfs:label>
    </owl:NamedIndividual>
    


    <!-- http://purl.obolibrary.org/obo/GAZ_00006941 -->

    <owl:NamedIndividual rdf:about="http://purl.obolibrary.org/obo/GAZ_00006941">
        <obo:RO_0001025 rdf:resource="http://purl.obolibrary.org/obo/GAZ_00006936"/>
        <oboInOwl:hasOBONamespace>GAZ</oboInOwl:hasOBONamespace>
        <oboInOwl:id>GAZ:00006941</oboInOwl:id>
        <rdfs:label>Umm an Nasan</rdfs:label>
    </owl:NamedIndividual>
    


    <!-- http://purl.obolibrary.org/obo/GAZ_00006942 -->

    <owl:NamedIndividual rdf:about="http://purl.obolibrary.org/obo/GAZ_00006942">
        <obo:RO_0001025 rdf:resource="http://purl.obolibrary.org/obo/GAZ_00006936"/>
        <obo:RO_0001025 rdf:resource="http://purl.obolibrary.org/obo/GAZ_00124888"/>
        <obo:IAO_0000115>An island in Bahrain. It lies in the Tubli Bay, east of Bahrain Island. It is connected to Bahrain Island and Sitra through the Sitra Causeway.</obo:IAO_0000115>
        <oboInOwl:hasOBONamespace>GAZ</oboInOwl:hasOBONamespace>
        <oboInOwl:id>GAZ:00006942</oboInOwl:id>
        <rdfs:label>Nabi Salah</rdfs:label>
    </owl:NamedIndividual>
    


    <!-- http://purl.obolibrary.org/obo/GAZ_00006943 -->

    <owl:NamedIndividual rdf:about="http://purl.obolibrary.org/obo/GAZ_00006943">
        <obo:RO_0001025 rdf:resource="http://purl.obolibrary.org/obo/GAZ_00006936"/>
        <oboInOwl:hasOBONamespace>GAZ</oboInOwl:hasOBONamespace>
        <oboInOwl:id>GAZ:00006943</oboInOwl:id>
        <rdfs:label>Jiddah</rdfs:label>
    </owl:NamedIndividual>
    


    <!-- http://purl.obolibrary.org/obo/GAZ_00006944 -->

    <owl:NamedIndividual rdf:about="http://purl.obolibrary.org/obo/GAZ_00006944">
        <obo:RO_0001025 rdf:resource="http://purl.obolibrary.org/obo/GAZ_00078661"/>
        <obo:IAO_0000115>The largest of the Hawar Islands of Bahrain.</obo:IAO_0000115>
        <oboInOwl:hasOBONamespace>GAZ</oboInOwl:hasOBONamespace>
        <oboInOwl:id>GAZ:00006944</oboInOwl:id>
        <rdfs:label>Hawar</rdfs:label>
    </owl:NamedIndividual>
    


    <!-- http://purl.obolibrary.org/obo/GAZ_00006945 -->

    <owl:NamedIndividual rdf:about="http://purl.obolibrary.org/obo/GAZ_00006945">
        <obo:RO_0001025 rdf:resource="http://purl.obolibrary.org/obo/GAZ_00006936"/>
        <obo:IAO_0000115>A group of man-made islands located in the northeast of Bahrain, near the coast of Muharraq island.</obo:IAO_0000115>
        <oboInOwl:hasOBONamespace>GAZ</oboInOwl:hasOBONamespace>
        <oboInOwl:id>GAZ:00006945</oboInOwl:id>
        <rdfs:label>Amwaj Islands</rdfs:label>
    </owl:NamedIndividual>
    


    <!-- http://purl.obolibrary.org/obo/GAZ_00006946 -->

    <owl:NamedIndividual rdf:about="http://purl.obolibrary.org/obo/GAZ_00006946">
        <obo:RO_0001025 rdf:resource="http://purl.obolibrary.org/obo/GAZ_00005295"/>
        <obo:RO_0001025 rdf:resource="http://purl.obolibrary.org/obo/GAZ_00015058"/>
        <obo:IAO_0000115>An island in the Persian Gulf. It extends from Ras Tanura in the north to Qatif in the west. It also is connected to Qatif by two causeways.</obo:IAO_0000115>
        <oboInOwl:hasOBONamespace>GAZ</oboInOwl:hasOBONamespace>
        <oboInOwl:id>GAZ:00006946</oboInOwl:id>
        <rdfs:label>Tarout Island</rdfs:label>
    </owl:NamedIndividual>
    


    <!-- http://purl.obolibrary.org/obo/GAZ_00007506 -->

    <owl:NamedIndividual rdf:about="http://purl.obolibrary.org/obo/GAZ_00007506"/>
    


    <!-- http://purl.obolibrary.org/obo/GAZ_00007507 -->

    <owl:NamedIndividual rdf:about="http://purl.obolibrary.org/obo/GAZ_00007507">
        <obo:RO_0001025 rdf:resource="http://purl.obolibrary.org/obo/GAZ_00031304"/>
    </owl:NamedIndividual>
    


    <!-- http://purl.obolibrary.org/obo/GAZ_00007508 -->

    <owl:NamedIndividual rdf:about="http://purl.obolibrary.org/obo/GAZ_00007508">
        <obo:RO_0001025 rdf:resource="http://purl.obolibrary.org/obo/GAZ_00005279"/>
    </owl:NamedIndividual>
    


    <!-- http://purl.obolibrary.org/obo/GAZ_00007509 -->

    <owl:NamedIndividual rdf:about="http://purl.obolibrary.org/obo/GAZ_00007509">
        <obo:RO_0001025 rdf:resource="http://purl.obolibrary.org/obo/GAZ_00005279"/>
    </owl:NamedIndividual>
    


    <!-- http://purl.obolibrary.org/obo/GAZ_00007862 -->

    <owl:NamedIndividual rdf:about="http://purl.obolibrary.org/obo/GAZ_00007862">
        <rdf:type rdf:resource="http://purl.obolibrary.org/obo/ENVO_00000032"/>
        <obo:IAO_0000115>A gulf situated northeastward and adjacent to the Red Sea, bounded by the coasts of Sinai Peninsula and Arabian Peninsula. Its southern limit with the Red Sea (in the Strait of T Degrees r Degrees n) is the following: A line joining Cape Al Qa Degrees bah (28 Degrees 01430 Seconds N - 34 Degrees 37 Minutes 15 Seconds E), in Saudi Arabia, southwestward to position 27 Degrees 58 Minutes 10 Seconds N - 34 Degrees 35 Minutes E) on the coast of T Degrees r Degrees n Island; thence from this position southward, through T Degrees r Degrees n Island, to its southwestern extremity (27 Degrees 54 Minutes 50 Seconds N - 34 Degrees 33 Minutes E); and thence from the southwestern extremity of T Degrees r Degrees n Island westward, along the parallel of 27 Degrees 54 Minutes 50 Seconds N, to the coast of Sinai Peninsula, in Egypt.</obo:IAO_0000115>
        <oboInOwl:hasOBONamespace>GAZ</oboInOwl:hasOBONamespace>
        <oboInOwl:id>GAZ:00007862</oboInOwl:id>
        <rdfs:label>Gulf of Aqaba</rdfs:label>
    </owl:NamedIndividual>
    


    <!-- http://purl.obolibrary.org/obo/GAZ_00008153 -->

    <owl:NamedIndividual rdf:about="http://purl.obolibrary.org/obo/GAZ_00008153">
        <rdf:type rdf:resource="http://purl.obolibrary.org/obo/ENVO_00000033"/>
        <obo:RO_0001025 rdf:resource="http://purl.obolibrary.org/obo/GAZ_00002456"/>
        <obo:IAO_0000115>A submarine basin. A pool of hot saline brine at the bottom of the central rift in the Red Sea.</obo:IAO_0000115>
        <oboInOwl:hasOBONamespace>GAZ</oboInOwl:hasOBONamespace>
        <oboInOwl:id>GAZ:00008153</oboInOwl:id>
        <rdfs:label>Atlantis II Deep</rdfs:label>
    </owl:NamedIndividual>
    


    <!-- http://purl.obolibrary.org/obo/GAZ_00009408 -->

    <owl:NamedIndividual rdf:about="http://purl.obolibrary.org/obo/GAZ_00009408">
        <obo:RO_0001025 rdf:resource="http://purl.obolibrary.org/obo/GAZ_00002456"/>
        <oboInOwl:hasOBONamespace>GAZ</oboInOwl:hasOBONamespace>
        <oboInOwl:id>GAZ:00009408</oboInOwl:id>
        <rdfs:label>Suakin Archipelago</rdfs:label>
    </owl:NamedIndividual>
    


    <!-- http://purl.obolibrary.org/obo/GAZ_00009519 -->

    <owl:NamedIndividual rdf:about="http://purl.obolibrary.org/obo/GAZ_00009519">
        <obo:RO_0001025 rdf:resource="http://purl.obolibrary.org/obo/GAZ_00005281"/>
    </owl:NamedIndividual>
    


    <!-- http://purl.obolibrary.org/obo/GAZ_00009683 -->

    <owl:NamedIndividual rdf:about="http://purl.obolibrary.org/obo/GAZ_00009683">
        <rdf:type rdf:resource="http://purl.obolibrary.org/obo/ENVO_00000220"/>
        <obo:RO_0001025 rdf:resource="http://purl.obolibrary.org/obo/GAZ_00002456"/>
        <obo:IAO_0000115>An island group located in the Red Sea near Massawa, Eritrea. It consists of two large and 124 small islands.</obo:IAO_0000115>
        <oboInOwl:hasOBONamespace>GAZ</oboInOwl:hasOBONamespace>
        <oboInOwl:id>GAZ:00009683</oboInOwl:id>
        <rdfs:label>Dahlak Archipelago</rdfs:label>
    </owl:NamedIndividual>
    


    <!-- http://purl.obolibrary.org/obo/GAZ_00010395 -->

    <owl:NamedIndividual rdf:about="http://purl.obolibrary.org/obo/GAZ_00010395"/>
    


    <!-- http://purl.obolibrary.org/obo/GAZ_00010396 -->

    <owl:NamedIndividual rdf:about="http://purl.obolibrary.org/obo/GAZ_00010396">
        <obo:RO_0001025 rdf:resource="http://purl.obolibrary.org/obo/GAZ_00031253"/>
    </owl:NamedIndividual>
    


    <!-- http://purl.obolibrary.org/obo/GAZ_00010397 -->

    <owl:NamedIndividual rdf:about="http://purl.obolibrary.org/obo/GAZ_00010397"/>
    


    <!-- http://purl.obolibrary.org/obo/GAZ_00010398 -->

    <owl:NamedIndividual rdf:about="http://purl.obolibrary.org/obo/GAZ_00010398"/>
    


    <!-- http://purl.obolibrary.org/obo/GAZ_00010399 -->

    <owl:NamedIndividual rdf:about="http://purl.obolibrary.org/obo/GAZ_00010399">
        <obo:RO_0001025 rdf:resource="http://purl.obolibrary.org/obo/GAZ_00007506"/>
        <obo:IAO_0000115>A populated place.</obo:IAO_0000115>
        <oboInOwl:hasOBONamespace>GAZ</oboInOwl:hasOBONamespace>
        <oboInOwl:id>GAZ:00010399</oboInOwl:id>
        <rdfs:label>Al Quenfadah</rdfs:label>
    </owl:NamedIndividual>
    


    <!-- http://purl.obolibrary.org/obo/GAZ_00014012 -->

    <owl:NamedIndividual rdf:about="http://purl.obolibrary.org/obo/GAZ_00014012">
        <obo:IAO_0000115>A volcanic field that lies in the Haurun-Druze Plateau in SW Syria near the border with Jordan. The most prominent feature of this volcanic field is 1800 m high Jabal ad Druze (also known variously as Djebel Al-Arab, Jabal ed Duruz, Jabal al Druz, Jebel Duraz, Djebel ed Drouz). The alkaline volcanic field consists of a group of 118 basaltic volcanoes active from the lower-Pleistocene to the Holocene. The large SW Plateau depression is filled by basaltic lava flows from volcanoes aligned in a NW-SE direction. This volcanic field lies within the northern part of the massive alkaline Harrat Ash Shaam volcanic field that extends from southern Syria through NW Jordan to Saudi Arabia.</obo:IAO_0000115>
        <oboInOwl:hasOBONamespace>GAZ</oboInOwl:hasOBONamespace>
        <oboInOwl:id>GAZ:00014012</oboInOwl:id>
        <rdfs:label>Jabal ad-Duruz Volcanic Field</rdfs:label>
    </owl:NamedIndividual>
    


    <!-- http://purl.obolibrary.org/obo/GAZ_00015054 -->

    <owl:NamedIndividual rdf:about="http://purl.obolibrary.org/obo/GAZ_00015054"/>
    


    <!-- http://purl.obolibrary.org/obo/GAZ_00015055 -->

    <owl:NamedIndividual rdf:about="http://purl.obolibrary.org/obo/GAZ_00015055"/>
    


    <!-- http://purl.obolibrary.org/obo/GAZ_00015056 -->

    <owl:NamedIndividual rdf:about="http://purl.obolibrary.org/obo/GAZ_00015056"/>
    


    <!-- http://purl.obolibrary.org/obo/GAZ_00015057 -->

    <owl:NamedIndividual rdf:about="http://purl.obolibrary.org/obo/GAZ_00015057"/>
    


    <!-- http://purl.obolibrary.org/obo/GAZ_00015058 -->

    <owl:NamedIndividual rdf:about="http://purl.obolibrary.org/obo/GAZ_00015058"/>
    


    <!-- http://purl.obolibrary.org/obo/GAZ_00015059 -->

    <owl:NamedIndividual rdf:about="http://purl.obolibrary.org/obo/GAZ_00015059"/>
    


    <!-- http://purl.obolibrary.org/obo/GAZ_00015060 -->

    <owl:NamedIndividual rdf:about="http://purl.obolibrary.org/obo/GAZ_00015060"/>
    


    <!-- http://purl.obolibrary.org/obo/GAZ_00015061 -->

    <owl:NamedIndividual rdf:about="http://purl.obolibrary.org/obo/GAZ_00015061"/>
    


    <!-- http://purl.obolibrary.org/obo/GAZ_00015062 -->

    <owl:NamedIndividual rdf:about="http://purl.obolibrary.org/obo/GAZ_00015062"/>
    


    <!-- http://purl.obolibrary.org/obo/GAZ_00018501 -->

    <owl:NamedIndividual rdf:about="http://purl.obolibrary.org/obo/GAZ_00018501">
        <obo:RO_0001025 rdf:resource="http://purl.obolibrary.org/obo/GAZ_00005295"/>
        <oboInOwl:hasOBONamespace>GAZ</oboInOwl:hasOBONamespace>
        <oboInOwl:id>GAZ:00018501</oboInOwl:id>
        <rdfs:label>Kuwait Bay</rdfs:label>
    </owl:NamedIndividual>
    


    <!-- http://purl.obolibrary.org/obo/GAZ_00018502 -->

    <owl:NamedIndividual rdf:about="http://purl.obolibrary.org/obo/GAZ_00018502">
        <obo:RO_0001025 rdf:resource="http://purl.obolibrary.org/obo/GAZ_00005295"/>
        <obo:IAO_0000115>An island in the Persian Gulf.</obo:IAO_0000115>
        <oboInOwl:hasOBONamespace>GAZ</oboInOwl:hasOBONamespace>
        <oboInOwl:id>GAZ:00018502</oboInOwl:id>
        <rdfs:label>Shomali Island</rdfs:label>
    </owl:NamedIndividual>
    


    <!-- http://purl.obolibrary.org/obo/GAZ_00018503 -->

    <owl:NamedIndividual rdf:about="http://purl.obolibrary.org/obo/GAZ_00018503">
        <obo:RO_0001025 rdf:resource="http://purl.obolibrary.org/obo/GAZ_00005295"/>
        <obo:IAO_0000115>An island in the Persian Gulf.</obo:IAO_0000115>
        <oboInOwl:hasOBONamespace>GAZ</oboInOwl:hasOBONamespace>
        <oboInOwl:id>GAZ:00018503</oboInOwl:id>
        <rdfs:label>Smaller Bent Island</rdfs:label>
    </owl:NamedIndividual>
    


    <!-- http://purl.obolibrary.org/obo/GAZ_00018504 -->

    <owl:NamedIndividual rdf:about="http://purl.obolibrary.org/obo/GAZ_00018504">
        <obo:RO_0001025 rdf:resource="http://purl.obolibrary.org/obo/GAZ_00005295"/>
        <obo:IAO_0000115>An island situated in the Strait of Hormuz off the south coast of Iran and east of the Persian Gulf.</obo:IAO_0000115>
        <oboInOwl:hasOBONamespace>GAZ</oboInOwl:hasOBONamespace>
        <oboInOwl:id>GAZ:00018504</oboInOwl:id>
        <rdfs:label>Qeshm Island</rdfs:label>
    </owl:NamedIndividual>
    


    <!-- http://purl.obolibrary.org/obo/GAZ_00018505 -->

    <owl:NamedIndividual rdf:about="http://purl.obolibrary.org/obo/GAZ_00018505">
        <obo:RO_0001025 rdf:resource="http://purl.obolibrary.org/obo/GAZ_00005295"/>
        <obo:IAO_0000115>An island in the Persian Gulf.</obo:IAO_0000115>
        <oboInOwl:hasOBONamespace>GAZ</oboInOwl:hasOBONamespace>
        <oboInOwl:id>GAZ:00018505</oboInOwl:id>
        <rdfs:label>Shatvar Island</rdfs:label>
    </owl:NamedIndividual>
    


    <!-- http://purl.obolibrary.org/obo/GAZ_00018506 -->

    <owl:NamedIndividual rdf:about="http://purl.obolibrary.org/obo/GAZ_00018506">
        <obo:RO_0001025 rdf:resource="http://purl.obolibrary.org/obo/GAZ_00005295"/>
        <obo:IAO_0000115>An island in the Persian Gulf.</obo:IAO_0000115>
        <oboInOwl:hasOBONamespace>GAZ</oboInOwl:hasOBONamespace>
        <oboInOwl:id>GAZ:00018506</oboInOwl:id>
        <rdfs:label>Shetor Island</rdfs:label>
    </owl:NamedIndividual>
    


    <!-- http://purl.obolibrary.org/obo/GAZ_00018507 -->

    <owl:NamedIndividual rdf:about="http://purl.obolibrary.org/obo/GAZ_00018507">
        <obo:RO_0001025 rdf:resource="http://purl.obolibrary.org/obo/GAZ_00005295"/>
        <obo:IAO_0000115>An island in the Persian Gulf.</obo:IAO_0000115>
        <oboInOwl:hasOBONamespace>GAZ</oboInOwl:hasOBONamespace>
        <oboInOwl:id>GAZ:00018507</oboInOwl:id>
        <rdfs:label>Qabre Nakhoda Island</rdfs:label>
    </owl:NamedIndividual>
    


    <!-- http://purl.obolibrary.org/obo/GAZ_00018508 -->

    <owl:NamedIndividual rdf:about="http://purl.obolibrary.org/obo/GAZ_00018508">
        <obo:RO_0001025 rdf:resource="http://purl.obolibrary.org/obo/GAZ_00005295"/>
        <obo:IAO_0000115>An island in the Persian Gulf.</obo:IAO_0000115>
        <oboInOwl:hasOBONamespace>GAZ</oboInOwl:hasOBONamespace>
        <oboInOwl:id>GAZ:00018508</oboInOwl:id>
        <rdfs:label>Rostam Island</rdfs:label>
    </owl:NamedIndividual>
    


    <!-- http://purl.obolibrary.org/obo/GAZ_00018509 -->

    <owl:NamedIndividual rdf:about="http://purl.obolibrary.org/obo/GAZ_00018509">
        <obo:RO_0001025 rdf:resource="http://purl.obolibrary.org/obo/GAZ_00250913"/>
        <obo:IAO_0000115>An island in the Persian Gulf.</obo:IAO_0000115>
        <oboInOwl:hasOBONamespace>GAZ</oboInOwl:hasOBONamespace>
        <oboInOwl:id>GAZ:00018509</oboInOwl:id>
        <rdfs:label>Shif Island</rdfs:label>
    </owl:NamedIndividual>
    


    <!-- http://purl.obolibrary.org/obo/GAZ_00018510 -->

    <owl:NamedIndividual rdf:about="http://purl.obolibrary.org/obo/GAZ_00018510">
        <obo:RO_0001025 rdf:resource="http://purl.obolibrary.org/obo/GAZ_00005295"/>
        <obo:IAO_0000115>An island in the Persian Gulf.</obo:IAO_0000115>
        <oboInOwl:hasOBONamespace>GAZ</oboInOwl:hasOBONamespace>
        <oboInOwl:id>GAZ:00018510</oboInOwl:id>
        <rdfs:label>Sirri Island</rdfs:label>
    </owl:NamedIndividual>
    


    <!-- http://purl.obolibrary.org/obo/GAZ_00018511 -->

    <owl:NamedIndividual rdf:about="http://purl.obolibrary.org/obo/GAZ_00018511">
        <obo:RO_0001025 rdf:resource="http://purl.obolibrary.org/obo/GAZ_00005295"/>
        <obo:IAO_0000115>An island in the Persian Gulf.</obo:IAO_0000115>
        <oboInOwl:hasOBONamespace>GAZ</oboInOwl:hasOBONamespace>
        <oboInOwl:id>GAZ:00018511</oboInOwl:id>
        <rdfs:label>Jonobi Island</rdfs:label>
    </owl:NamedIndividual>
    


    <!-- http://purl.obolibrary.org/obo/GAZ_00018512 -->

    <owl:NamedIndividual rdf:about="http://purl.obolibrary.org/obo/GAZ_00018512">
        <obo:RO_0001025 rdf:resource="http://purl.obolibrary.org/obo/GAZ_00005295"/>
        <obo:IAO_0000115>An Iranian island in the Persian Gulf.</obo:IAO_0000115>
        <oboInOwl:hasOBONamespace>GAZ</oboInOwl:hasOBONamespace>
        <oboInOwl:id>GAZ:00018512</oboInOwl:id>
        <rdfs:label>Farsi Island</rdfs:label>
    </owl:NamedIndividual>
    


    <!-- http://purl.obolibrary.org/obo/GAZ_00018513 -->

    <owl:NamedIndividual rdf:about="http://purl.obolibrary.org/obo/GAZ_00018513">
        <obo:RO_0001025 rdf:resource="http://purl.obolibrary.org/obo/GAZ_00250921"/>
        <obo:IAO_0000115>An island in the Persian Gulf.</obo:IAO_0000115>
        <oboInOwl:hasOBONamespace>GAZ</oboInOwl:hasOBONamespace>
        <oboInOwl:id>GAZ:00018513</oboInOwl:id>
        <rdfs:label>Jazireh-ye Forur</rdfs:label>
    </owl:NamedIndividual>
    


    <!-- http://purl.obolibrary.org/obo/GAZ_00018514 -->

    <owl:NamedIndividual rdf:about="http://purl.obolibrary.org/obo/GAZ_00018514">
        <obo:RO_0001025 rdf:resource="http://purl.obolibrary.org/obo/GAZ_00005295"/>
        <obo:IAO_0000115>A resort island in the Persian Gulf. It is part of the Hormozgan Province of Iran.</obo:IAO_0000115>
        <oboInOwl:hasOBONamespace>GAZ</oboInOwl:hasOBONamespace>
        <oboInOwl:id>GAZ:00018514</oboInOwl:id>
        <rdfs:label>Kish Island</rdfs:label>
    </owl:NamedIndividual>
    


    <!-- http://purl.obolibrary.org/obo/GAZ_00018515 -->

    <owl:NamedIndividual rdf:about="http://purl.obolibrary.org/obo/GAZ_00018515">
        <obo:RO_0001025 rdf:resource="http://purl.obolibrary.org/obo/GAZ_00005295"/>
        <obo:IAO_0000115>An island off the coast of Iran in the Persian Gulf.</obo:IAO_0000115>
        <oboInOwl:hasOBONamespace>GAZ</oboInOwl:hasOBONamespace>
        <oboInOwl:id>GAZ:00018515</oboInOwl:id>
        <rdfs:label>Larak Island</rdfs:label>
    </owl:NamedIndividual>
    


    <!-- http://purl.obolibrary.org/obo/GAZ_00018516 -->

    <owl:NamedIndividual rdf:about="http://purl.obolibrary.org/obo/GAZ_00018516">
        <obo:RO_0001025 rdf:resource="http://purl.obolibrary.org/obo/GAZ_00005295"/>
        <obo:IAO_0000115>An Iranian island in the Persian Gulf.</obo:IAO_0000115>
        <oboInOwl:hasOBONamespace>GAZ</oboInOwl:hasOBONamespace>
        <oboInOwl:id>GAZ:00018516</oboInOwl:id>
        <rdfs:label>Lavan Island</rdfs:label>
    </owl:NamedIndividual>
    


    <!-- http://purl.obolibrary.org/obo/GAZ_00018517 -->

    <owl:NamedIndividual rdf:about="http://purl.obolibrary.org/obo/GAZ_00018517">
        <obo:RO_0001025 rdf:resource="http://purl.obolibrary.org/obo/GAZ_00005295"/>
        <obo:IAO_0000115>A continental island in the Persian Gulf belonging to Iran.</obo:IAO_0000115>
        <oboInOwl:hasOBONamespace>GAZ</oboInOwl:hasOBONamespace>
        <oboInOwl:id>GAZ:00018517</oboInOwl:id>
        <rdfs:label>Kharg Island</rdfs:label>
    </owl:NamedIndividual>
    


    <!-- http://purl.obolibrary.org/obo/GAZ_00018518 -->

    <owl:NamedIndividual rdf:about="http://purl.obolibrary.org/obo/GAZ_00018518">
        <obo:RO_0001025 rdf:resource="http://purl.obolibrary.org/obo/GAZ_00005295"/>
        <obo:IAO_0000115>An Iranian island in the Persian Gulf. It is part of the Khuzestan province in southwestern Iran and is close to the city of Abadan.</obo:IAO_0000115>
        <oboInOwl:hasOBONamespace>GAZ</oboInOwl:hasOBONamespace>
        <oboInOwl:id>GAZ:00018518</oboInOwl:id>
        <rdfs:label>Minu Island</rdfs:label>
    </owl:NamedIndividual>
    


    <!-- http://purl.obolibrary.org/obo/GAZ_00018519 -->

    <owl:NamedIndividual rdf:about="http://purl.obolibrary.org/obo/GAZ_00018519">
        <obo:RO_0001025 rdf:resource="http://purl.obolibrary.org/obo/GAZ_00005295"/>
        <obo:IAO_0000115>An island in the Persian Gulf.</obo:IAO_0000115>
        <oboInOwl:hasOBONamespace>GAZ</oboInOwl:hasOBONamespace>
        <oboInOwl:id>GAZ:00018519</oboInOwl:id>
        <rdfs:label>Omolkarm Island</rdfs:label>
    </owl:NamedIndividual>
    


    <!-- http://purl.obolibrary.org/obo/GAZ_00018520 -->

    <owl:NamedIndividual rdf:about="http://purl.obolibrary.org/obo/GAZ_00018520">
        <obo:RO_0001025 rdf:resource="http://purl.obolibrary.org/obo/GAZ_00005295"/>
        <obo:IAO_0000115>An island.</obo:IAO_0000115>
        <oboInOwl:hasOBONamespace>GAZ</oboInOwl:hasOBONamespace>
        <oboInOwl:id>GAZ:00018520</oboInOwl:id>
        <rdfs:label>Dara Island</rdfs:label>
    </owl:NamedIndividual>
    


    <!-- http://purl.obolibrary.org/obo/GAZ_00018521 -->

    <owl:NamedIndividual rdf:about="http://purl.obolibrary.org/obo/GAZ_00018521">
        <obo:RO_0001025 rdf:resource="http://purl.obolibrary.org/obo/GAZ_00005295"/>
        <obo:IAO_0000115>An island located on the eastern side of the Persian Gulf, part of a six-island archipelago near the entrance to the Strait of Hormuz.</obo:IAO_0000115>
        <oboInOwl:hasOBONamespace>GAZ</oboInOwl:hasOBONamespace>
        <oboInOwl:id>GAZ:00018521</oboInOwl:id>
        <rdfs:label>Abu Musa Island</rdfs:label>
    </owl:NamedIndividual>
    


    <!-- http://purl.obolibrary.org/obo/GAZ_00018522 -->

    <owl:NamedIndividual rdf:about="http://purl.obolibrary.org/obo/GAZ_00018522">
        <obo:RO_0001025 rdf:resource="http://purl.obolibrary.org/obo/GAZ_00005295"/>
        <oboInOwl:hasOBONamespace>GAZ</oboInOwl:hasOBONamespace>
        <oboInOwl:id>GAZ:00018522</oboInOwl:id>
        <rdfs:label>Abbasak Island</rdfs:label>
    </owl:NamedIndividual>
    


    <!-- http://purl.obolibrary.org/obo/GAZ_00018523 -->

    <owl:NamedIndividual rdf:about="http://purl.obolibrary.org/obo/GAZ_00018523">
        <obo:RO_0001025 rdf:resource="http://purl.obolibrary.org/obo/GAZ_00005295"/>
        <obo:IAO_0000115>An island in the N Persian Gulf.</obo:IAO_0000115>
        <oboInOwl:hasOBONamespace>GAZ</oboInOwl:hasOBONamespace>
        <oboInOwl:id>GAZ:00018523</oboInOwl:id>
        <rdfs:label>Buneh Island</rdfs:label>
    </owl:NamedIndividual>
    


    <!-- http://purl.obolibrary.org/obo/GAZ_00018524 -->

    <owl:NamedIndividual rdf:about="http://purl.obolibrary.org/obo/GAZ_00018524">
        <obo:RO_0001025 rdf:resource="http://purl.obolibrary.org/obo/GAZ_00005295"/>
        <obo:IAO_0000115>An island located in the straight of Hormuz and is part of the Hormozgan Province.</obo:IAO_0000115>
        <oboInOwl:hasOBONamespace>GAZ</oboInOwl:hasOBONamespace>
        <oboInOwl:id>GAZ:00018524</oboInOwl:id>
        <rdfs:label>Hormuz Island</rdfs:label>
    </owl:NamedIndividual>
    


    <!-- http://purl.obolibrary.org/obo/GAZ_00018525 -->

    <owl:NamedIndividual rdf:about="http://purl.obolibrary.org/obo/GAZ_00018525">
        <obo:RO_0001025 rdf:resource="http://purl.obolibrary.org/obo/GAZ_00005295"/>
        <obo:IAO_0000115>Two small islands in the eastern Persian Gulf, close to the Strait of Hormuz, some 12 km from each other and 20 south of the Iranian island of Qeshm.</obo:IAO_0000115>
        <oboInOwl:hasOBONamespace>GAZ</oboInOwl:hasOBONamespace>
        <oboInOwl:id>GAZ:00018525</oboInOwl:id>
        <rdfs:label>Greater and Lesser Tunbs</rdfs:label>
    </owl:NamedIndividual>
    


    <!-- http://purl.obolibrary.org/obo/GAZ_00018526 -->

    <owl:NamedIndividual rdf:about="http://purl.obolibrary.org/obo/GAZ_00018526">
        <obo:RO_0001025 rdf:resource="http://purl.obolibrary.org/obo/GAZ_00005295"/>
        <obo:IAO_0000115>An island in the Persian Gulf, located in Hormozgan Province, to the west of Kish Island and due south of Bastak.</obo:IAO_0000115>
        <oboInOwl:hasOBONamespace>GAZ</oboInOwl:hasOBONamespace>
        <oboInOwl:id>GAZ:00018526</oboInOwl:id>
        <rdfs:label>Hendurabi Island</rdfs:label>
    </owl:NamedIndividual>
    


    <!-- http://purl.obolibrary.org/obo/GAZ_00018527 -->

    <owl:NamedIndividual rdf:about="http://purl.obolibrary.org/obo/GAZ_00018527">
        <obo:RO_0001025 rdf:resource="http://purl.obolibrary.org/obo/GAZ_00005295"/>
        <obo:IAO_0000115>An island in the Persian Gulf.</obo:IAO_0000115>
        <oboInOwl:hasOBONamespace>GAZ</oboInOwl:hasOBONamespace>
        <oboInOwl:id>GAZ:00018527</oboInOwl:id>
        <rdfs:label>Germ Island</rdfs:label>
    </owl:NamedIndividual>
    


    <!-- http://purl.obolibrary.org/obo/GAZ_00018528 -->

    <owl:NamedIndividual rdf:about="http://purl.obolibrary.org/obo/GAZ_00018528">
        <obo:RO_0001025 rdf:resource="http://purl.obolibrary.org/obo/GAZ_00005295"/>
        <obo:IAO_0000115>An island in the Persian Gulf.</obo:IAO_0000115>
        <oboInOwl:hasOBONamespace>GAZ</oboInOwl:hasOBONamespace>
        <oboInOwl:id>GAZ:00018528</oboInOwl:id>
        <rdfs:label>Hengam Island</rdfs:label>
    </owl:NamedIndividual>
    


    <!-- http://purl.obolibrary.org/obo/GAZ_00018529 -->

    <owl:NamedIndividual rdf:about="http://purl.obolibrary.org/obo/GAZ_00018529">
        <obo:RO_0001025 rdf:resource="http://purl.obolibrary.org/obo/GAZ_00250921"/>
        <obo:IAO_0000115>An island in the Persian Gulf.</obo:IAO_0000115>
        <oboInOwl:hasOBONamespace>GAZ</oboInOwl:hasOBONamespace>
        <oboInOwl:id>GAZ:00018529</oboInOwl:id>
        <rdfs:label>Jazireh-ye Bani Forur</rdfs:label>
    </owl:NamedIndividual>
    


    <!-- http://purl.obolibrary.org/obo/GAZ_00018530 -->

    <owl:NamedIndividual rdf:about="http://purl.obolibrary.org/obo/GAZ_00018530">
        <obo:RO_0001025 rdf:resource="http://purl.obolibrary.org/obo/GAZ_00005295"/>
        <obo:IAO_0000115>An island in the Persian Gulf.</obo:IAO_0000115>
        <oboInOwl:hasOBONamespace>GAZ</oboInOwl:hasOBONamespace>
        <oboInOwl:id>GAZ:00018530</oboInOwl:id>
        <rdfs:label>Forurgan Island</rdfs:label>
    </owl:NamedIndividual>
    


    <!-- http://purl.obolibrary.org/obo/GAZ_00018532 -->

    <owl:NamedIndividual rdf:about="http://purl.obolibrary.org/obo/GAZ_00018532">
        <obo:RO_0001025 rdf:resource="http://purl.obolibrary.org/obo/GAZ_00005295"/>
        <oboInOwl:hasOBONamespace>GAZ</oboInOwl:hasOBONamespace>
        <oboInOwl:id>GAZ:00018532</oboInOwl:id>
        <rdfs:label>Northern mudflat islands</rdfs:label>
    </owl:NamedIndividual>
    


    <!-- http://purl.obolibrary.org/obo/GAZ_00018533 -->

    <owl:NamedIndividual rdf:about="http://purl.obolibrary.org/obo/GAZ_00018533">
        <obo:RO_0001025 rdf:resource="http://purl.obolibrary.org/obo/GAZ_00005295"/>
        <oboInOwl:hasOBONamespace>GAZ</oboInOwl:hasOBONamespace>
        <oboInOwl:id>GAZ:00018533</oboInOwl:id>
        <rdfs:label>Failaka Islands</rdfs:label>
    </owl:NamedIndividual>
    


    <!-- http://purl.obolibrary.org/obo/GAZ_00018534 -->

    <owl:NamedIndividual rdf:about="http://purl.obolibrary.org/obo/GAZ_00018534">
        <obo:RO_0001025 rdf:resource="http://purl.obolibrary.org/obo/GAZ_00005295"/>
        <oboInOwl:hasOBONamespace>GAZ</oboInOwl:hasOBONamespace>
        <oboInOwl:id>GAZ:00018534</oboInOwl:id>
        <rdfs:label>Southern Islands</rdfs:label>
    </owl:NamedIndividual>
    


    <!-- http://purl.obolibrary.org/obo/GAZ_00018535 -->

    <owl:NamedIndividual rdf:about="http://purl.obolibrary.org/obo/GAZ_00018535">
        <obo:RO_0001025 rdf:resource="http://purl.obolibrary.org/obo/GAZ_00018532"/>
        <oboInOwl:hasOBONamespace>GAZ</oboInOwl:hasOBONamespace>
        <oboInOwl:id>GAZ:00018535</oboInOwl:id>
        <rdfs:label>Bubiyan Island</rdfs:label>
    </owl:NamedIndividual>
    


    <!-- http://purl.obolibrary.org/obo/GAZ_00018536 -->

    <owl:NamedIndividual rdf:about="http://purl.obolibrary.org/obo/GAZ_00018536">
        <obo:RO_0001025 rdf:resource="http://purl.obolibrary.org/obo/GAZ_00018532"/>
        <oboInOwl:hasOBONamespace>GAZ</oboInOwl:hasOBONamespace>
        <oboInOwl:id>GAZ:00018536</oboInOwl:id>
        <rdfs:label>Warbah Island</rdfs:label>
    </owl:NamedIndividual>
    


    <!-- http://purl.obolibrary.org/obo/GAZ_00018537 -->

    <owl:NamedIndividual rdf:about="http://purl.obolibrary.org/obo/GAZ_00018537">
        <obo:RO_0001025 rdf:resource="http://purl.obolibrary.org/obo/GAZ_00018533"/>
        <oboInOwl:hasOBONamespace>GAZ</oboInOwl:hasOBONamespace>
        <oboInOwl:id>GAZ:00018537</oboInOwl:id>
        <rdfs:label>Auhah Island</rdfs:label>
    </owl:NamedIndividual>
    


    <!-- http://purl.obolibrary.org/obo/GAZ_00018538 -->

    <owl:NamedIndividual rdf:about="http://purl.obolibrary.org/obo/GAZ_00018538">
        <obo:RO_0001025 rdf:resource="http://purl.obolibrary.org/obo/GAZ_00018533"/>
        <oboInOwl:hasOBONamespace>GAZ</oboInOwl:hasOBONamespace>
        <oboInOwl:id>GAZ:00018538</oboInOwl:id>
        <rdfs:label>Failaka Island</rdfs:label>
    </owl:NamedIndividual>
    


    <!-- http://purl.obolibrary.org/obo/GAZ_00018539 -->

    <owl:NamedIndividual rdf:about="http://purl.obolibrary.org/obo/GAZ_00018539">
        <obo:RO_0001025 rdf:resource="http://purl.obolibrary.org/obo/GAZ_00018533"/>
        <oboInOwl:hasOBONamespace>GAZ</oboInOwl:hasOBONamespace>
        <oboInOwl:id>GAZ:00018539</oboInOwl:id>
        <rdfs:label>Miskan Island</rdfs:label>
    </owl:NamedIndividual>
    


    <!-- http://purl.obolibrary.org/obo/GAZ_00018540 -->

    <owl:NamedIndividual rdf:about="http://purl.obolibrary.org/obo/GAZ_00018540">
        <obo:RO_0001025 rdf:resource="http://purl.obolibrary.org/obo/GAZ_00018501"/>
        <oboInOwl:hasOBONamespace>GAZ</oboInOwl:hasOBONamespace>
        <oboInOwl:id>GAZ:00018540</oboInOwl:id>
        <rdfs:label>Shuwaikh Island</rdfs:label>
    </owl:NamedIndividual>
    


    <!-- http://purl.obolibrary.org/obo/GAZ_00018541 -->

    <owl:NamedIndividual rdf:about="http://purl.obolibrary.org/obo/GAZ_00018541">
        <obo:RO_0001025 rdf:resource="http://purl.obolibrary.org/obo/GAZ_00018501"/>
        <oboInOwl:hasOBONamespace>GAZ</oboInOwl:hasOBONamespace>
        <oboInOwl:id>GAZ:00018541</oboInOwl:id>
        <rdfs:label>Umm an Namil Island</rdfs:label>
    </owl:NamedIndividual>
    


    <!-- http://purl.obolibrary.org/obo/GAZ_00018542 -->

    <owl:NamedIndividual rdf:about="http://purl.obolibrary.org/obo/GAZ_00018542">
        <obo:RO_0001025 rdf:resource="http://purl.obolibrary.org/obo/GAZ_00018534"/>
        <oboInOwl:hasOBONamespace>GAZ</oboInOwl:hasOBONamespace>
        <oboInOwl:id>GAZ:00018542</oboInOwl:id>
        <rdfs:label>Umm al Maradim Island</rdfs:label>
    </owl:NamedIndividual>
    


    <!-- http://purl.obolibrary.org/obo/GAZ_00018543 -->

    <owl:NamedIndividual rdf:about="http://purl.obolibrary.org/obo/GAZ_00018543">
        <obo:RO_0001025 rdf:resource="http://purl.obolibrary.org/obo/GAZ_00018534"/>
        <obo:IAO_0000115>A small offshore island with associated coral reefs in the northern Gulf.</obo:IAO_0000115>
        <oboInOwl:hasOBONamespace>GAZ</oboInOwl:hasOBONamespace>
        <oboInOwl:id>GAZ:00018543</oboInOwl:id>
        <rdfs:label>Kubbar Island</rdfs:label>
    </owl:NamedIndividual>
    


    <!-- http://purl.obolibrary.org/obo/GAZ_00018544 -->

    <owl:NamedIndividual rdf:about="http://purl.obolibrary.org/obo/GAZ_00018544">
        <obo:RO_0001025 rdf:resource="http://purl.obolibrary.org/obo/GAZ_00018534"/>
        <oboInOwl:hasOBONamespace>GAZ</oboInOwl:hasOBONamespace>
        <oboInOwl:id>GAZ:00018544</oboInOwl:id>
        <rdfs:label>Qaruh Island</rdfs:label>
    </owl:NamedIndividual>
    


    <!-- http://purl.obolibrary.org/obo/GAZ_00031211 -->

    <owl:NamedIndividual rdf:about="http://purl.obolibrary.org/obo/GAZ_00031211">
        <obo:RO_0001025 rdf:resource="http://purl.obolibrary.org/obo/GAZ_00015062"/>
        <oboInOwl:hasOBONamespace>GAZ</oboInOwl:hasOBONamespace>
        <oboInOwl:id>GAZ:00031211</oboInOwl:id>
        <rdfs:label>Governorate of Al-Bahah</rdfs:label>
    </owl:NamedIndividual>
    


    <!-- http://purl.obolibrary.org/obo/GAZ_00031212 -->

    <owl:NamedIndividual rdf:about="http://purl.obolibrary.org/obo/GAZ_00031212">
        <obo:RO_0001025 rdf:resource="http://purl.obolibrary.org/obo/GAZ_00015062"/>
        <oboInOwl:hasOBONamespace>GAZ</oboInOwl:hasOBONamespace>
        <oboInOwl:id>GAZ:00031212</oboInOwl:id>
        <rdfs:label>Governorate of Al-Mandaq</rdfs:label>
    </owl:NamedIndividual>
    


    <!-- http://purl.obolibrary.org/obo/GAZ_00031213 -->

    <owl:NamedIndividual rdf:about="http://purl.obolibrary.org/obo/GAZ_00031213">
        <obo:RO_0001025 rdf:resource="http://purl.obolibrary.org/obo/GAZ_00015062"/>
        <oboInOwl:hasOBONamespace>GAZ</oboInOwl:hasOBONamespace>
        <oboInOwl:id>GAZ:00031213</oboInOwl:id>
        <rdfs:label>Governorate of Biljurashi</rdfs:label>
    </owl:NamedIndividual>
    


    <!-- http://purl.obolibrary.org/obo/GAZ_00031214 -->

    <owl:NamedIndividual rdf:about="http://purl.obolibrary.org/obo/GAZ_00031214">
        <obo:RO_0001025 rdf:resource="http://purl.obolibrary.org/obo/GAZ_00015062"/>
        <oboInOwl:hasOBONamespace>GAZ</oboInOwl:hasOBONamespace>
        <oboInOwl:id>GAZ:00031214</oboInOwl:id>
        <rdfs:label>Governorate of Al-Mukhwah</rdfs:label>
    </owl:NamedIndividual>
    


    <!-- http://purl.obolibrary.org/obo/GAZ_00031215 -->

    <owl:NamedIndividual rdf:about="http://purl.obolibrary.org/obo/GAZ_00031215">
        <obo:RO_0001025 rdf:resource="http://purl.obolibrary.org/obo/GAZ_00015062"/>
        <oboInOwl:hasOBONamespace>GAZ</oboInOwl:hasOBONamespace>
        <oboInOwl:id>GAZ:00031215</oboInOwl:id>
        <rdfs:label>Governorate of Al-Qari</rdfs:label>
    </owl:NamedIndividual>
    


    <!-- http://purl.obolibrary.org/obo/GAZ_00031216 -->

    <owl:NamedIndividual rdf:about="http://purl.obolibrary.org/obo/GAZ_00031216">
        <obo:RO_0001025 rdf:resource="http://purl.obolibrary.org/obo/GAZ_00015062"/>
        <oboInOwl:hasOBONamespace>GAZ</oboInOwl:hasOBONamespace>
        <oboInOwl:id>GAZ:00031216</oboInOwl:id>
        <rdfs:label>Governorate of Qilwah</rdfs:label>
    </owl:NamedIndividual>
    


    <!-- http://purl.obolibrary.org/obo/GAZ_00031217 -->

    <owl:NamedIndividual rdf:about="http://purl.obolibrary.org/obo/GAZ_00031217">
        <obo:RO_0001025 rdf:resource="http://purl.obolibrary.org/obo/GAZ_00015062"/>
        <oboInOwl:hasOBONamespace>GAZ</oboInOwl:hasOBONamespace>
        <oboInOwl:id>GAZ:00031217</oboInOwl:id>
        <rdfs:label>Governorate of Al-Aqiq</rdfs:label>
    </owl:NamedIndividual>
    


    <!-- http://purl.obolibrary.org/obo/GAZ_00031218 -->

    <owl:NamedIndividual rdf:about="http://purl.obolibrary.org/obo/GAZ_00031218">
        <obo:RO_0001025 rdf:resource="http://purl.obolibrary.org/obo/GAZ_00015059"/>
        <oboInOwl:hasOBONamespace>GAZ</oboInOwl:hasOBONamespace>
        <oboInOwl:id>GAZ:00031218</oboInOwl:id>
        <rdfs:label>Governorate of Dawamat al-Jandal</rdfs:label>
    </owl:NamedIndividual>
    


    <!-- http://purl.obolibrary.org/obo/GAZ_00031219 -->

    <owl:NamedIndividual rdf:about="http://purl.obolibrary.org/obo/GAZ_00031219">
        <obo:RO_0001025 rdf:resource="http://purl.obolibrary.org/obo/GAZ_00015057"/>
        <oboInOwl:hasOBONamespace>GAZ</oboInOwl:hasOBONamespace>
        <oboInOwl:id>GAZ:00031219</oboInOwl:id>
        <rdfs:label>Governorate of Rafha</rdfs:label>
    </owl:NamedIndividual>
    


    <!-- http://purl.obolibrary.org/obo/GAZ_00031220 -->

    <owl:NamedIndividual rdf:about="http://purl.obolibrary.org/obo/GAZ_00031220">
        <obo:RO_0001025 rdf:resource="http://purl.obolibrary.org/obo/GAZ_00015057"/>
        <oboInOwl:hasOBONamespace>GAZ</oboInOwl:hasOBONamespace>
        <oboInOwl:id>GAZ:00031220</oboInOwl:id>
        <rdfs:label>Governorate of Ar&apos;ar</rdfs:label>
    </owl:NamedIndividual>
    


    <!-- http://purl.obolibrary.org/obo/GAZ_00031221 -->

    <owl:NamedIndividual rdf:about="http://purl.obolibrary.org/obo/GAZ_00031221">
        <obo:RO_0001025 rdf:resource="http://purl.obolibrary.org/obo/GAZ_00015056"/>
        <oboInOwl:hasOBONamespace>GAZ</oboInOwl:hasOBONamespace>
        <oboInOwl:id>GAZ:00031221</oboInOwl:id>
        <rdfs:label>Governorate of Badr al-Janub</rdfs:label>
    </owl:NamedIndividual>
    


    <!-- http://purl.obolibrary.org/obo/GAZ_00031222 -->

    <owl:NamedIndividual rdf:about="http://purl.obolibrary.org/obo/GAZ_00031222">
        <obo:RO_0001025 rdf:resource="http://purl.obolibrary.org/obo/GAZ_00015057"/>
        <oboInOwl:hasOBONamespace>GAZ</oboInOwl:hasOBONamespace>
        <oboInOwl:id>GAZ:00031222</oboInOwl:id>
        <rdfs:label>Governorate of Turayf</rdfs:label>
    </owl:NamedIndividual>
    


    <!-- http://purl.obolibrary.org/obo/GAZ_00031223 -->

    <owl:NamedIndividual rdf:about="http://purl.obolibrary.org/obo/GAZ_00031223">
        <obo:RO_0001025 rdf:resource="http://purl.obolibrary.org/obo/GAZ_00015059"/>
        <oboInOwl:hasOBONamespace>GAZ</oboInOwl:hasOBONamespace>
        <oboInOwl:id>GAZ:00031223</oboInOwl:id>
        <rdfs:label>Governorate of Al-Qurayyat</rdfs:label>
    </owl:NamedIndividual>
    


    <!-- http://purl.obolibrary.org/obo/GAZ_00031224 -->

    <owl:NamedIndividual rdf:about="http://purl.obolibrary.org/obo/GAZ_00031224">
        <obo:RO_0001025 rdf:resource="http://purl.obolibrary.org/obo/GAZ_00015059"/>
        <oboInOwl:hasOBONamespace>GAZ</oboInOwl:hasOBONamespace>
        <oboInOwl:id>GAZ:00031224</oboInOwl:id>
        <rdfs:label>Governorate of Sakaka</rdfs:label>
    </owl:NamedIndividual>
    


    <!-- http://purl.obolibrary.org/obo/GAZ_00031225 -->

    <owl:NamedIndividual rdf:about="http://purl.obolibrary.org/obo/GAZ_00031225">
        <obo:RO_0001025 rdf:resource="http://purl.obolibrary.org/obo/GAZ_00015055"/>
        <oboInOwl:hasOBONamespace>GAZ</oboInOwl:hasOBONamespace>
        <oboInOwl:id>GAZ:00031225</oboInOwl:id>
        <rdfs:label>Governorate of Al-Asyah</rdfs:label>
    </owl:NamedIndividual>
    


    <!-- http://purl.obolibrary.org/obo/GAZ_00031226 -->

    <owl:NamedIndividual rdf:about="http://purl.obolibrary.org/obo/GAZ_00031226">
        <obo:RO_0001025 rdf:resource="http://purl.obolibrary.org/obo/GAZ_00015055"/>
        <oboInOwl:hasOBONamespace>GAZ</oboInOwl:hasOBONamespace>
        <oboInOwl:id>GAZ:00031226</oboInOwl:id>
        <rdfs:label>Governorate of Al-Badai</rdfs:label>
    </owl:NamedIndividual>
    


    <!-- http://purl.obolibrary.org/obo/GAZ_00031227 -->

    <owl:NamedIndividual rdf:about="http://purl.obolibrary.org/obo/GAZ_00031227">
        <obo:RO_0001025 rdf:resource="http://purl.obolibrary.org/obo/GAZ_00015055"/>
        <oboInOwl:hasOBONamespace>GAZ</oboInOwl:hasOBONamespace>
        <oboInOwl:id>GAZ:00031227</oboInOwl:id>
        <rdfs:label>Governorate of Ar-Rass</rdfs:label>
    </owl:NamedIndividual>
    


    <!-- http://purl.obolibrary.org/obo/GAZ_00031228 -->

    <owl:NamedIndividual rdf:about="http://purl.obolibrary.org/obo/GAZ_00031228">
        <obo:RO_0001025 rdf:resource="http://purl.obolibrary.org/obo/GAZ_00015055"/>
        <oboInOwl:hasOBONamespace>GAZ</oboInOwl:hasOBONamespace>
        <oboInOwl:id>GAZ:00031228</oboInOwl:id>
        <rdfs:label>Governorate of Riyadh al-Khabra</rdfs:label>
    </owl:NamedIndividual>
    


    <!-- http://purl.obolibrary.org/obo/GAZ_00031229 -->

    <owl:NamedIndividual rdf:about="http://purl.obolibrary.org/obo/GAZ_00031229">
        <obo:RO_0001025 rdf:resource="http://purl.obolibrary.org/obo/GAZ_00015055"/>
        <oboInOwl:hasOBONamespace>GAZ</oboInOwl:hasOBONamespace>
        <oboInOwl:id>GAZ:00031229</oboInOwl:id>
        <rdfs:label>Governorate of Ash-Shimasiyah</rdfs:label>
    </owl:NamedIndividual>
    


    <!-- http://purl.obolibrary.org/obo/GAZ_00031230 -->

    <owl:NamedIndividual rdf:about="http://purl.obolibrary.org/obo/GAZ_00031230">
        <obo:RO_0001025 rdf:resource="http://purl.obolibrary.org/obo/GAZ_00015055"/>
        <oboInOwl:hasOBONamespace>GAZ</oboInOwl:hasOBONamespace>
        <oboInOwl:id>GAZ:00031230</oboInOwl:id>
        <rdfs:label>Governorate of Unayzah</rdfs:label>
    </owl:NamedIndividual>
    


    <!-- http://purl.obolibrary.org/obo/GAZ_00031231 -->

    <owl:NamedIndividual rdf:about="http://purl.obolibrary.org/obo/GAZ_00031231">
        <obo:RO_0001025 rdf:resource="http://purl.obolibrary.org/obo/GAZ_00015055"/>
        <oboInOwl:hasOBONamespace>GAZ</oboInOwl:hasOBONamespace>
        <oboInOwl:id>GAZ:00031231</oboInOwl:id>
        <rdfs:label>Governorate of Uyun al-Jiwa</rdfs:label>
    </owl:NamedIndividual>
    


    <!-- http://purl.obolibrary.org/obo/GAZ_00031232 -->

    <owl:NamedIndividual rdf:about="http://purl.obolibrary.org/obo/GAZ_00031232">
        <obo:RO_0001025 rdf:resource="http://purl.obolibrary.org/obo/GAZ_00015055"/>
        <oboInOwl:hasOBONamespace>GAZ</oboInOwl:hasOBONamespace>
        <oboInOwl:id>GAZ:00031232</oboInOwl:id>
        <rdfs:label>Governorate of Al-Bukayriyah</rdfs:label>
    </owl:NamedIndividual>
    


    <!-- http://purl.obolibrary.org/obo/GAZ_00031233 -->

    <owl:NamedIndividual rdf:about="http://purl.obolibrary.org/obo/GAZ_00031233">
        <obo:RO_0001025 rdf:resource="http://purl.obolibrary.org/obo/GAZ_00015055"/>
        <oboInOwl:hasOBONamespace>GAZ</oboInOwl:hasOBONamespace>
        <oboInOwl:id>GAZ:00031233</oboInOwl:id>
        <rdfs:label>Governorate of Buraydah</rdfs:label>
    </owl:NamedIndividual>
    


    <!-- http://purl.obolibrary.org/obo/GAZ_00031234 -->

    <owl:NamedIndividual rdf:about="http://purl.obolibrary.org/obo/GAZ_00031234">
        <obo:RO_0001025 rdf:resource="http://purl.obolibrary.org/obo/GAZ_00015055"/>
        <oboInOwl:hasOBONamespace>GAZ</oboInOwl:hasOBONamespace>
        <oboInOwl:id>GAZ:00031234</oboInOwl:id>
        <rdfs:label>Governorate of Al-Midhnab</rdfs:label>
    </owl:NamedIndividual>
    


    <!-- http://purl.obolibrary.org/obo/GAZ_00031235 -->

    <owl:NamedIndividual rdf:about="http://purl.obolibrary.org/obo/GAZ_00031235">
        <obo:RO_0001025 rdf:resource="http://purl.obolibrary.org/obo/GAZ_00015055"/>
        <oboInOwl:hasOBONamespace>GAZ</oboInOwl:hasOBONamespace>
        <oboInOwl:id>GAZ:00031235</oboInOwl:id>
        <rdfs:label>Governorate of An-Nabhaniyah</rdfs:label>
    </owl:NamedIndividual>
    


    <!-- http://purl.obolibrary.org/obo/GAZ_00031236 -->

    <owl:NamedIndividual rdf:about="http://purl.obolibrary.org/obo/GAZ_00031236">
        <obo:RO_0001025 rdf:resource="http://purl.obolibrary.org/obo/GAZ_00010395"/>
        <oboInOwl:hasOBONamespace>GAZ</oboInOwl:hasOBONamespace>
        <oboInOwl:id>GAZ:00031236</oboInOwl:id>
        <rdfs:label>Governorate of Afif</rdfs:label>
    </owl:NamedIndividual>
    


    <!-- http://purl.obolibrary.org/obo/GAZ_00031237 -->

    <owl:NamedIndividual rdf:about="http://purl.obolibrary.org/obo/GAZ_00031237">
        <obo:RO_0001025 rdf:resource="http://purl.obolibrary.org/obo/GAZ_00010395"/>
        <oboInOwl:hasOBONamespace>GAZ</oboInOwl:hasOBONamespace>
        <oboInOwl:id>GAZ:00031237</oboInOwl:id>
        <rdfs:label>Governorate of Al-Aflaj</rdfs:label>
    </owl:NamedIndividual>
    


    <!-- http://purl.obolibrary.org/obo/GAZ_00031238 -->

    <owl:NamedIndividual rdf:about="http://purl.obolibrary.org/obo/GAZ_00031238">
        <obo:RO_0001025 rdf:resource="http://purl.obolibrary.org/obo/GAZ_00010395"/>
        <oboInOwl:hasOBONamespace>GAZ</oboInOwl:hasOBONamespace>
        <oboInOwl:id>GAZ:00031238</oboInOwl:id>
        <rdfs:label>Governorate of Ad-Diriyah</rdfs:label>
    </owl:NamedIndividual>
    


    <!-- http://purl.obolibrary.org/obo/GAZ_00031239 -->

    <owl:NamedIndividual rdf:about="http://purl.obolibrary.org/obo/GAZ_00031239">
        <obo:RO_0001025 rdf:resource="http://purl.obolibrary.org/obo/GAZ_00010395"/>
        <oboInOwl:hasOBONamespace>GAZ</oboInOwl:hasOBONamespace>
        <oboInOwl:id>GAZ:00031239</oboInOwl:id>
        <rdfs:label>Governorate of Duruma</rdfs:label>
    </owl:NamedIndividual>
    


    <!-- http://purl.obolibrary.org/obo/GAZ_00031240 -->

    <owl:NamedIndividual rdf:about="http://purl.obolibrary.org/obo/GAZ_00031240">
        <obo:RO_0001025 rdf:resource="http://purl.obolibrary.org/obo/GAZ_00010395"/>
        <oboInOwl:hasOBONamespace>GAZ</oboInOwl:hasOBONamespace>
        <oboInOwl:id>GAZ:00031240</oboInOwl:id>
        <rdfs:label>Governorate of Ad-Duwadimi</rdfs:label>
    </owl:NamedIndividual>
    


    <!-- http://purl.obolibrary.org/obo/GAZ_00031241 -->

    <owl:NamedIndividual rdf:about="http://purl.obolibrary.org/obo/GAZ_00031241">
        <obo:RO_0001025 rdf:resource="http://purl.obolibrary.org/obo/GAZ_00010395"/>
        <oboInOwl:hasOBONamespace>GAZ</oboInOwl:hasOBONamespace>
        <oboInOwl:id>GAZ:00031241</oboInOwl:id>
        <rdfs:label>Governorate of Al-Ghat</rdfs:label>
    </owl:NamedIndividual>
    


    <!-- http://purl.obolibrary.org/obo/GAZ_00031242 -->

    <owl:NamedIndividual rdf:about="http://purl.obolibrary.org/obo/GAZ_00031242">
        <obo:RO_0001025 rdf:resource="http://purl.obolibrary.org/obo/GAZ_00010395"/>
        <oboInOwl:hasOBONamespace>GAZ</oboInOwl:hasOBONamespace>
        <oboInOwl:id>GAZ:00031242</oboInOwl:id>
        <rdfs:label>Governorate of Hawtat Bani Tamim</rdfs:label>
    </owl:NamedIndividual>
    


    <!-- http://purl.obolibrary.org/obo/GAZ_00031243 -->

    <owl:NamedIndividual rdf:about="http://purl.obolibrary.org/obo/GAZ_00031243">
        <obo:RO_0001025 rdf:resource="http://purl.obolibrary.org/obo/GAZ_00010395"/>
        <oboInOwl:hasOBONamespace>GAZ</oboInOwl:hasOBONamespace>
        <oboInOwl:id>GAZ:00031243</oboInOwl:id>
        <rdfs:label>Governorate of Al-Kharj</rdfs:label>
    </owl:NamedIndividual>
    


    <!-- http://purl.obolibrary.org/obo/GAZ_00031244 -->

    <owl:NamedIndividual rdf:about="http://purl.obolibrary.org/obo/GAZ_00031244">
        <obo:RO_0001025 rdf:resource="http://purl.obolibrary.org/obo/GAZ_00010395"/>
        <oboInOwl:hasOBONamespace>GAZ</oboInOwl:hasOBONamespace>
        <oboInOwl:id>GAZ:00031244</oboInOwl:id>
        <rdfs:label>Governorate of Al-Muzahimiya</rdfs:label>
    </owl:NamedIndividual>
    


    <!-- http://purl.obolibrary.org/obo/GAZ_00031245 -->

    <owl:NamedIndividual rdf:about="http://purl.obolibrary.org/obo/GAZ_00031245">
        <obo:RO_0001025 rdf:resource="http://purl.obolibrary.org/obo/GAZ_00010395"/>
        <oboInOwl:hasOBONamespace>GAZ</oboInOwl:hasOBONamespace>
        <oboInOwl:id>GAZ:00031245</oboInOwl:id>
        <rdfs:label>Governorate of Al-Majmaah</rdfs:label>
    </owl:NamedIndividual>
    


    <!-- http://purl.obolibrary.org/obo/GAZ_00031246 -->

    <owl:NamedIndividual rdf:about="http://purl.obolibrary.org/obo/GAZ_00031246">
        <obo:RO_0001025 rdf:resource="http://purl.obolibrary.org/obo/GAZ_00010395"/>
        <oboInOwl:hasOBONamespace>GAZ</oboInOwl:hasOBONamespace>
        <oboInOwl:id>GAZ:00031246</oboInOwl:id>
        <rdfs:label>Governorate of Huraymila</rdfs:label>
    </owl:NamedIndividual>
    


    <!-- http://purl.obolibrary.org/obo/GAZ_00031247 -->

    <owl:NamedIndividual rdf:about="http://purl.obolibrary.org/obo/GAZ_00031247">
        <obo:RO_0001025 rdf:resource="http://purl.obolibrary.org/obo/GAZ_00010395"/>
        <oboInOwl:hasOBONamespace>GAZ</oboInOwl:hasOBONamespace>
        <oboInOwl:id>GAZ:00031247</oboInOwl:id>
        <rdfs:label>Governorate of Al-Quwayiyah</rdfs:label>
    </owl:NamedIndividual>
    


    <!-- http://purl.obolibrary.org/obo/GAZ_00031248 -->

    <owl:NamedIndividual rdf:about="http://purl.obolibrary.org/obo/GAZ_00031248">
        <obo:RO_0001025 rdf:resource="http://purl.obolibrary.org/obo/GAZ_00010395"/>
        <oboInOwl:hasOBONamespace>GAZ</oboInOwl:hasOBONamespace>
        <oboInOwl:id>GAZ:00031248</oboInOwl:id>
        <rdfs:label>Governorate of Al-Hariq</rdfs:label>
    </owl:NamedIndividual>
    


    <!-- http://purl.obolibrary.org/obo/GAZ_00031249 -->

    <owl:NamedIndividual rdf:about="http://purl.obolibrary.org/obo/GAZ_00031249">
        <obo:RO_0001025 rdf:resource="http://purl.obolibrary.org/obo/GAZ_00010395"/>
        <oboInOwl:hasOBONamespace>GAZ</oboInOwl:hasOBONamespace>
        <oboInOwl:id>GAZ:00031249</oboInOwl:id>
        <rdfs:label>Governorate of Shaqra</rdfs:label>
    </owl:NamedIndividual>
    


    <!-- http://purl.obolibrary.org/obo/GAZ_00031250 -->

    <owl:NamedIndividual rdf:about="http://purl.obolibrary.org/obo/GAZ_00031250">
        <obo:RO_0001025 rdf:resource="http://purl.obolibrary.org/obo/GAZ_00010395"/>
        <oboInOwl:hasOBONamespace>GAZ</oboInOwl:hasOBONamespace>
        <oboInOwl:id>GAZ:00031250</oboInOwl:id>
        <rdfs:label>Governorate of Thadiq</rdfs:label>
    </owl:NamedIndividual>
    


    <!-- http://purl.obolibrary.org/obo/GAZ_00031251 -->

    <owl:NamedIndividual rdf:about="http://purl.obolibrary.org/obo/GAZ_00031251">
        <obo:RO_0001025 rdf:resource="http://purl.obolibrary.org/obo/GAZ_00010395"/>
        <oboInOwl:hasOBONamespace>GAZ</oboInOwl:hasOBONamespace>
        <oboInOwl:id>GAZ:00031251</oboInOwl:id>
        <rdfs:label>Governorate of Rumah</rdfs:label>
    </owl:NamedIndividual>
    


    <!-- http://purl.obolibrary.org/obo/GAZ_00031252 -->

    <owl:NamedIndividual rdf:about="http://purl.obolibrary.org/obo/GAZ_00031252">
        <obo:RO_0001025 rdf:resource="http://purl.obolibrary.org/obo/GAZ_00010395"/>
        <oboInOwl:hasOBONamespace>GAZ</oboInOwl:hasOBONamespace>
        <oboInOwl:id>GAZ:00031252</oboInOwl:id>
        <rdfs:label>Governorate of As-Sulayyil</rdfs:label>
    </owl:NamedIndividual>
    


    <!-- http://purl.obolibrary.org/obo/GAZ_00031253 -->

    <owl:NamedIndividual rdf:about="http://purl.obolibrary.org/obo/GAZ_00031253">
        <obo:RO_0001025 rdf:resource="http://purl.obolibrary.org/obo/GAZ_00010395"/>
        <oboInOwl:hasOBONamespace>GAZ</oboInOwl:hasOBONamespace>
        <oboInOwl:id>GAZ:00031253</oboInOwl:id>
        <rdfs:label>Governorate of Ar-Riyad</rdfs:label>
    </owl:NamedIndividual>
    


    <!-- http://purl.obolibrary.org/obo/GAZ_00031254 -->

    <owl:NamedIndividual rdf:about="http://purl.obolibrary.org/obo/GAZ_00031254">
        <obo:RO_0001025 rdf:resource="http://purl.obolibrary.org/obo/GAZ_00010395"/>
        <oboInOwl:hasOBONamespace>GAZ</oboInOwl:hasOBONamespace>
        <oboInOwl:id>GAZ:00031254</oboInOwl:id>
        <rdfs:label>Governorate of Wadi ad-Dwasir</rdfs:label>
    </owl:NamedIndividual>
    


    <!-- http://purl.obolibrary.org/obo/GAZ_00031255 -->

    <owl:NamedIndividual rdf:about="http://purl.obolibrary.org/obo/GAZ_00031255">
        <obo:RO_0001025 rdf:resource="http://purl.obolibrary.org/obo/GAZ_00010395"/>
        <oboInOwl:hasOBONamespace>GAZ</oboInOwl:hasOBONamespace>
        <oboInOwl:id>GAZ:00031255</oboInOwl:id>
        <rdfs:label>Governorate of Az-Zulfi</rdfs:label>
    </owl:NamedIndividual>
    


    <!-- http://purl.obolibrary.org/obo/GAZ_00031256 -->

    <owl:NamedIndividual rdf:about="http://purl.obolibrary.org/obo/GAZ_00031256">
        <obo:RO_0001025 rdf:resource="http://purl.obolibrary.org/obo/GAZ_00010397"/>
        <oboInOwl:hasOBONamespace>GAZ</oboInOwl:hasOBONamespace>
        <oboInOwl:id>GAZ:00031256</oboInOwl:id>
        <rdfs:label>Governorate of Al-Majardah</rdfs:label>
    </owl:NamedIndividual>
    


    <!-- http://purl.obolibrary.org/obo/GAZ_00031257 -->

    <owl:NamedIndividual rdf:about="http://purl.obolibrary.org/obo/GAZ_00031257">
        <obo:RO_0001025 rdf:resource="http://purl.obolibrary.org/obo/GAZ_00010397"/>
        <oboInOwl:hasOBONamespace>GAZ</oboInOwl:hasOBONamespace>
        <oboInOwl:id>GAZ:00031257</oboInOwl:id>
        <rdfs:label>Governorate of Bishah</rdfs:label>
    </owl:NamedIndividual>
    


    <!-- http://purl.obolibrary.org/obo/GAZ_00031258 -->

    <owl:NamedIndividual rdf:about="http://purl.obolibrary.org/obo/GAZ_00031258">
        <obo:RO_0001025 rdf:resource="http://purl.obolibrary.org/obo/GAZ_00010397"/>
        <oboInOwl:hasOBONamespace>GAZ</oboInOwl:hasOBONamespace>
        <oboInOwl:id>GAZ:00031258</oboInOwl:id>
        <rdfs:label>Governorate of Rijal alma</rdfs:label>
    </owl:NamedIndividual>
    


    <!-- http://purl.obolibrary.org/obo/GAZ_00031259 -->

    <owl:NamedIndividual rdf:about="http://purl.obolibrary.org/obo/GAZ_00031259">
        <obo:RO_0001025 rdf:resource="http://purl.obolibrary.org/obo/GAZ_00010397"/>
        <oboInOwl:hasOBONamespace>GAZ</oboInOwl:hasOBONamespace>
        <oboInOwl:id>GAZ:00031259</oboInOwl:id>
        <rdfs:label>Governorate of Balqarn</rdfs:label>
    </owl:NamedIndividual>
    


    <!-- http://purl.obolibrary.org/obo/GAZ_00031260 -->

    <owl:NamedIndividual rdf:about="http://purl.obolibrary.org/obo/GAZ_00031260">
        <obo:RO_0001025 rdf:resource="http://purl.obolibrary.org/obo/GAZ_00010397"/>
        <oboInOwl:hasOBONamespace>GAZ</oboInOwl:hasOBONamespace>
        <oboInOwl:id>GAZ:00031260</oboInOwl:id>
        <rdfs:label>Governorate of Muhayil</rdfs:label>
    </owl:NamedIndividual>
    


    <!-- http://purl.obolibrary.org/obo/GAZ_00031261 -->

    <owl:NamedIndividual rdf:about="http://purl.obolibrary.org/obo/GAZ_00031261">
        <obo:RO_0001025 rdf:resource="http://purl.obolibrary.org/obo/GAZ_00010397"/>
        <oboInOwl:hasOBONamespace>GAZ</oboInOwl:hasOBONamespace>
        <oboInOwl:id>GAZ:00031261</oboInOwl:id>
        <rdfs:label>Governorate of Ahd Rifaydah</rdfs:label>
    </owl:NamedIndividual>
    


    <!-- http://purl.obolibrary.org/obo/GAZ_00031262 -->

    <owl:NamedIndividual rdf:about="http://purl.obolibrary.org/obo/GAZ_00031262">
        <obo:RO_0001025 rdf:resource="http://purl.obolibrary.org/obo/GAZ_00010397"/>
        <oboInOwl:hasOBONamespace>GAZ</oboInOwl:hasOBONamespace>
        <oboInOwl:id>GAZ:00031262</oboInOwl:id>
        <rdfs:label>Governorate of Khamis Mushayt</rdfs:label>
    </owl:NamedIndividual>
    


    <!-- http://purl.obolibrary.org/obo/GAZ_00031263 -->

    <owl:NamedIndividual rdf:about="http://purl.obolibrary.org/obo/GAZ_00031263">
        <obo:RO_0001025 rdf:resource="http://purl.obolibrary.org/obo/GAZ_00010397"/>
        <oboInOwl:hasOBONamespace>GAZ</oboInOwl:hasOBONamespace>
        <oboInOwl:id>GAZ:00031263</oboInOwl:id>
        <rdfs:label>Governorate of An-Namas</rdfs:label>
    </owl:NamedIndividual>
    


    <!-- http://purl.obolibrary.org/obo/GAZ_00031264 -->

    <owl:NamedIndividual rdf:about="http://purl.obolibrary.org/obo/GAZ_00031264">
        <obo:RO_0001025 rdf:resource="http://purl.obolibrary.org/obo/GAZ_00010397"/>
        <oboInOwl:hasOBONamespace>GAZ</oboInOwl:hasOBONamespace>
        <oboInOwl:id>GAZ:00031264</oboInOwl:id>
        <rdfs:label>Governorate of Abha</rdfs:label>
    </owl:NamedIndividual>
    


    <!-- http://purl.obolibrary.org/obo/GAZ_00031265 -->

    <owl:NamedIndividual rdf:about="http://purl.obolibrary.org/obo/GAZ_00031265">
        <obo:RO_0001025 rdf:resource="http://purl.obolibrary.org/obo/GAZ_00010397"/>
        <oboInOwl:hasOBONamespace>GAZ</oboInOwl:hasOBONamespace>
        <oboInOwl:id>GAZ:00031265</oboInOwl:id>
        <rdfs:label>Governorate of Sarat Abidah</rdfs:label>
    </owl:NamedIndividual>
    


    <!-- http://purl.obolibrary.org/obo/GAZ_00031266 -->

    <owl:NamedIndividual rdf:about="http://purl.obolibrary.org/obo/GAZ_00031266">
        <obo:RO_0001025 rdf:resource="http://purl.obolibrary.org/obo/GAZ_00010397"/>
        <oboInOwl:hasOBONamespace>GAZ</oboInOwl:hasOBONamespace>
        <oboInOwl:id>GAZ:00031266</oboInOwl:id>
        <rdfs:label>Governorate of Tathlith</rdfs:label>
    </owl:NamedIndividual>
    


    <!-- http://purl.obolibrary.org/obo/GAZ_00031267 -->

    <owl:NamedIndividual rdf:about="http://purl.obolibrary.org/obo/GAZ_00031267">
        <obo:RO_0001025 rdf:resource="http://purl.obolibrary.org/obo/GAZ_00010397"/>
        <oboInOwl:hasOBONamespace>GAZ</oboInOwl:hasOBONamespace>
        <oboInOwl:id>GAZ:00031267</oboInOwl:id>
        <rdfs:label>Governorate of Zahran al-Janub</rdfs:label>
    </owl:NamedIndividual>
    


    <!-- http://purl.obolibrary.org/obo/GAZ_00031268 -->

    <owl:NamedIndividual rdf:about="http://purl.obolibrary.org/obo/GAZ_00031268">
        <obo:RO_0001025 rdf:resource="http://purl.obolibrary.org/obo/GAZ_00015061"/>
        <oboInOwl:hasOBONamespace>GAZ</oboInOwl:hasOBONamespace>
        <oboInOwl:id>GAZ:00031268</oboInOwl:id>
        <rdfs:label>Governorate of Baqa</rdfs:label>
    </owl:NamedIndividual>
    


    <!-- http://purl.obolibrary.org/obo/GAZ_00031269 -->

    <owl:NamedIndividual rdf:about="http://purl.obolibrary.org/obo/GAZ_00031269">
        <obo:RO_0001025 rdf:resource="http://purl.obolibrary.org/obo/GAZ_00015061"/>
        <oboInOwl:hasOBONamespace>GAZ</oboInOwl:hasOBONamespace>
        <oboInOwl:id>GAZ:00031269</oboInOwl:id>
        <rdfs:label>Governorate of Al-Ghazalah</rdfs:label>
    </owl:NamedIndividual>
    


    <!-- http://purl.obolibrary.org/obo/GAZ_00031270 -->

    <owl:NamedIndividual rdf:about="http://purl.obolibrary.org/obo/GAZ_00031270">
        <obo:RO_0001025 rdf:resource="http://purl.obolibrary.org/obo/GAZ_00015061"/>
        <oboInOwl:hasOBONamespace>GAZ</oboInOwl:hasOBONamespace>
        <oboInOwl:id>GAZ:00031270</oboInOwl:id>
        <rdfs:label>Governorate of Ha&apos;il</rdfs:label>
    </owl:NamedIndividual>
    


    <!-- http://purl.obolibrary.org/obo/GAZ_00031271 -->

    <owl:NamedIndividual rdf:about="http://purl.obolibrary.org/obo/GAZ_00031271">
        <obo:RO_0001025 rdf:resource="http://purl.obolibrary.org/obo/GAZ_00015061"/>
        <oboInOwl:hasOBONamespace>GAZ</oboInOwl:hasOBONamespace>
        <oboInOwl:id>GAZ:00031271</oboInOwl:id>
        <rdfs:label>Governorate of As-Shinan</rdfs:label>
    </owl:NamedIndividual>
    


    <!-- http://purl.obolibrary.org/obo/GAZ_00031272 -->

    <owl:NamedIndividual rdf:about="http://purl.obolibrary.org/obo/GAZ_00031272">
        <obo:RO_0001025 rdf:resource="http://purl.obolibrary.org/obo/GAZ_00015058"/>
        <oboInOwl:hasOBONamespace>GAZ</oboInOwl:hasOBONamespace>
        <oboInOwl:id>GAZ:00031272</oboInOwl:id>
        <rdfs:label>Governorate of Al-Ahsa</rdfs:label>
    </owl:NamedIndividual>
    


    <!-- http://purl.obolibrary.org/obo/GAZ_00031273 -->

    <owl:NamedIndividual rdf:about="http://purl.obolibrary.org/obo/GAZ_00031273">
        <obo:RO_0001025 rdf:resource="http://purl.obolibrary.org/obo/GAZ_00015058"/>
        <oboInOwl:hasOBONamespace>GAZ</oboInOwl:hasOBONamespace>
        <oboInOwl:id>GAZ:00031273</oboInOwl:id>
        <rdfs:label>Governorate of Buqayq</rdfs:label>
    </owl:NamedIndividual>
    


    <!-- http://purl.obolibrary.org/obo/GAZ_00031274 -->

    <owl:NamedIndividual rdf:about="http://purl.obolibrary.org/obo/GAZ_00031274">
        <obo:RO_0001025 rdf:resource="http://purl.obolibrary.org/obo/GAZ_00015058"/>
        <oboInOwl:hasOBONamespace>GAZ</oboInOwl:hasOBONamespace>
        <oboInOwl:id>GAZ:00031274</oboInOwl:id>
        <rdfs:label>Governorate of Ad-Dammam</rdfs:label>
    </owl:NamedIndividual>
    


    <!-- http://purl.obolibrary.org/obo/GAZ_00031275 -->

    <owl:NamedIndividual rdf:about="http://purl.obolibrary.org/obo/GAZ_00031275">
        <obo:RO_0001025 rdf:resource="http://purl.obolibrary.org/obo/GAZ_00015058"/>
        <oboInOwl:hasOBONamespace>GAZ</oboInOwl:hasOBONamespace>
        <oboInOwl:id>GAZ:00031275</oboInOwl:id>
        <rdfs:label>Governorate of Hafar al-Batin</rdfs:label>
    </owl:NamedIndividual>
    


    <!-- http://purl.obolibrary.org/obo/GAZ_00031276 -->

    <owl:NamedIndividual rdf:about="http://purl.obolibrary.org/obo/GAZ_00031276">
        <obo:RO_0001025 rdf:resource="http://purl.obolibrary.org/obo/GAZ_00015058"/>
        <oboInOwl:hasOBONamespace>GAZ</oboInOwl:hasOBONamespace>
        <oboInOwl:id>GAZ:00031276</oboInOwl:id>
        <rdfs:label>Governorate of Al-Jubayl</rdfs:label>
    </owl:NamedIndividual>
    


    <!-- http://purl.obolibrary.org/obo/GAZ_00031277 -->

    <owl:NamedIndividual rdf:about="http://purl.obolibrary.org/obo/GAZ_00031277">
        <obo:RO_0001025 rdf:resource="http://purl.obolibrary.org/obo/GAZ_00015058"/>
        <oboInOwl:hasOBONamespace>GAZ</oboInOwl:hasOBONamespace>
        <oboInOwl:id>GAZ:00031277</oboInOwl:id>
        <rdfs:label>Governorate of Al-Khafji</rdfs:label>
    </owl:NamedIndividual>
    


    <!-- http://purl.obolibrary.org/obo/GAZ_00031278 -->

    <owl:NamedIndividual rdf:about="http://purl.obolibrary.org/obo/GAZ_00031278">
        <obo:RO_0001025 rdf:resource="http://purl.obolibrary.org/obo/GAZ_00015058"/>
        <oboInOwl:hasOBONamespace>GAZ</oboInOwl:hasOBONamespace>
        <oboInOwl:id>GAZ:00031278</oboInOwl:id>
        <rdfs:label>Governorate of Al-Khubar</rdfs:label>
    </owl:NamedIndividual>
    


    <!-- http://purl.obolibrary.org/obo/GAZ_00031279 -->

    <owl:NamedIndividual rdf:about="http://purl.obolibrary.org/obo/GAZ_00031279">
        <obo:RO_0001025 rdf:resource="http://purl.obolibrary.org/obo/GAZ_00015058"/>
        <oboInOwl:hasOBONamespace>GAZ</oboInOwl:hasOBONamespace>
        <oboInOwl:id>GAZ:00031279</oboInOwl:id>
        <rdfs:label>Governorate of Al-Nuayriyah</rdfs:label>
    </owl:NamedIndividual>
    


    <!-- http://purl.obolibrary.org/obo/GAZ_00031280 -->

    <owl:NamedIndividual rdf:about="http://purl.obolibrary.org/obo/GAZ_00031280">
        <obo:RO_0001025 rdf:resource="http://purl.obolibrary.org/obo/GAZ_00015058"/>
        <oboInOwl:hasOBONamespace>GAZ</oboInOwl:hasOBONamespace>
        <oboInOwl:id>GAZ:00031280</oboInOwl:id>
        <rdfs:label>Governorate of Qaryah al-Ulya</rdfs:label>
    </owl:NamedIndividual>
    


    <!-- http://purl.obolibrary.org/obo/GAZ_00031281 -->

    <owl:NamedIndividual rdf:about="http://purl.obolibrary.org/obo/GAZ_00031281">
        <obo:RO_0001025 rdf:resource="http://purl.obolibrary.org/obo/GAZ_00015058"/>
        <oboInOwl:hasOBONamespace>GAZ</oboInOwl:hasOBONamespace>
        <oboInOwl:id>GAZ:00031281</oboInOwl:id>
        <rdfs:label>Governorate of Al-Qatif</rdfs:label>
    </owl:NamedIndividual>
    


    <!-- http://purl.obolibrary.org/obo/GAZ_00031282 -->

    <owl:NamedIndividual rdf:about="http://purl.obolibrary.org/obo/GAZ_00031282">
        <obo:RO_0001025 rdf:resource="http://purl.obolibrary.org/obo/GAZ_00015058"/>
        <oboInOwl:hasOBONamespace>GAZ</oboInOwl:hasOBONamespace>
        <oboInOwl:id>GAZ:00031282</oboInOwl:id>
        <rdfs:label>Governorate of Ras Tannurah</rdfs:label>
    </owl:NamedIndividual>
    


    <!-- http://purl.obolibrary.org/obo/GAZ_00031283 -->

    <owl:NamedIndividual rdf:about="http://purl.obolibrary.org/obo/GAZ_00031283">
        <obo:RO_0001025 rdf:resource="http://purl.obolibrary.org/obo/GAZ_00010398"/>
        <oboInOwl:hasOBONamespace>GAZ</oboInOwl:hasOBONamespace>
        <oboInOwl:id>GAZ:00031283</oboInOwl:id>
        <rdfs:label>Governorate of Abu Arish</rdfs:label>
    </owl:NamedIndividual>
    


    <!-- http://purl.obolibrary.org/obo/GAZ_00031284 -->

    <owl:NamedIndividual rdf:about="http://purl.obolibrary.org/obo/GAZ_00031284">
        <obo:RO_0001025 rdf:resource="http://purl.obolibrary.org/obo/GAZ_00010398"/>
        <oboInOwl:hasOBONamespace>GAZ</oboInOwl:hasOBONamespace>
        <oboInOwl:id>GAZ:00031284</oboInOwl:id>
        <rdfs:label>Governorate of Damad</rdfs:label>
    </owl:NamedIndividual>
    


    <!-- http://purl.obolibrary.org/obo/GAZ_00031285 -->

    <owl:NamedIndividual rdf:about="http://purl.obolibrary.org/obo/GAZ_00031285">
        <obo:RO_0001025 rdf:resource="http://purl.obolibrary.org/obo/GAZ_00010398"/>
        <oboInOwl:hasOBONamespace>GAZ</oboInOwl:hasOBONamespace>
        <oboInOwl:id>GAZ:00031285</oboInOwl:id>
        <rdfs:label>Governorate of Baysh</rdfs:label>
    </owl:NamedIndividual>
    


    <!-- http://purl.obolibrary.org/obo/GAZ_00031286 -->

    <owl:NamedIndividual rdf:about="http://purl.obolibrary.org/obo/GAZ_00031286">
        <obo:RO_0001025 rdf:resource="http://purl.obolibrary.org/obo/GAZ_00010398"/>
        <oboInOwl:hasOBONamespace>GAZ</oboInOwl:hasOBONamespace>
        <oboInOwl:id>GAZ:00031286</oboInOwl:id>
        <rdfs:label>Governorate of Farasan</rdfs:label>
    </owl:NamedIndividual>
    


    <!-- http://purl.obolibrary.org/obo/GAZ_00031287 -->

    <owl:NamedIndividual rdf:about="http://purl.obolibrary.org/obo/GAZ_00031287">
        <obo:RO_0001025 rdf:resource="http://purl.obolibrary.org/obo/GAZ_00010398"/>
        <oboInOwl:hasOBONamespace>GAZ</oboInOwl:hasOBONamespace>
        <oboInOwl:id>GAZ:00031287</oboInOwl:id>
        <rdfs:label>Governorate of Al-Darb</rdfs:label>
    </owl:NamedIndividual>
    


    <!-- http://purl.obolibrary.org/obo/GAZ_00031288 -->

    <owl:NamedIndividual rdf:about="http://purl.obolibrary.org/obo/GAZ_00031288">
        <obo:RO_0001025 rdf:resource="http://purl.obolibrary.org/obo/GAZ_00010398"/>
        <oboInOwl:hasOBONamespace>GAZ</oboInOwl:hasOBONamespace>
        <oboInOwl:id>GAZ:00031288</oboInOwl:id>
        <rdfs:label>Governorate of Al-Aridah</rdfs:label>
    </owl:NamedIndividual>
    


    <!-- http://purl.obolibrary.org/obo/GAZ_00031289 -->

    <owl:NamedIndividual rdf:about="http://purl.obolibrary.org/obo/GAZ_00031289">
        <obo:RO_0001025 rdf:resource="http://purl.obolibrary.org/obo/GAZ_00010398"/>
        <oboInOwl:hasOBONamespace>GAZ</oboInOwl:hasOBONamespace>
        <oboInOwl:id>GAZ:00031289</oboInOwl:id>
        <rdfs:label>Governorate of Al-Harth</rdfs:label>
    </owl:NamedIndividual>
    


    <!-- http://purl.obolibrary.org/obo/GAZ_00031290 -->

    <owl:NamedIndividual rdf:about="http://purl.obolibrary.org/obo/GAZ_00031290">
        <obo:RO_0001025 rdf:resource="http://purl.obolibrary.org/obo/GAZ_00010398"/>
        <oboInOwl:hasOBONamespace>GAZ</oboInOwl:hasOBONamespace>
        <oboInOwl:id>GAZ:00031290</oboInOwl:id>
        <rdfs:label>Governorate of Ad-Dair</rdfs:label>
    </owl:NamedIndividual>
    


    <!-- http://purl.obolibrary.org/obo/GAZ_00031291 -->

    <owl:NamedIndividual rdf:about="http://purl.obolibrary.org/obo/GAZ_00031291">
        <obo:RO_0001025 rdf:resource="http://purl.obolibrary.org/obo/GAZ_00010398"/>
        <oboInOwl:hasOBONamespace>GAZ</oboInOwl:hasOBONamespace>
        <oboInOwl:id>GAZ:00031291</oboInOwl:id>
        <rdfs:label>Governorate of Ahad al-Musarihah</rdfs:label>
    </owl:NamedIndividual>
    


    <!-- http://purl.obolibrary.org/obo/GAZ_00031292 -->

    <owl:NamedIndividual rdf:about="http://purl.obolibrary.org/obo/GAZ_00031292">
        <obo:RO_0001025 rdf:resource="http://purl.obolibrary.org/obo/GAZ_00010398"/>
        <oboInOwl:hasOBONamespace>GAZ</oboInOwl:hasOBONamespace>
        <oboInOwl:id>GAZ:00031292</oboInOwl:id>
        <rdfs:label>Governorate of Sabya</rdfs:label>
    </owl:NamedIndividual>
    


    <!-- http://purl.obolibrary.org/obo/GAZ_00031293 -->

    <owl:NamedIndividual rdf:about="http://purl.obolibrary.org/obo/GAZ_00031293">
        <obo:RO_0001025 rdf:resource="http://purl.obolibrary.org/obo/GAZ_00010398"/>
        <oboInOwl:hasOBONamespace>GAZ</oboInOwl:hasOBONamespace>
        <oboInOwl:id>GAZ:00031293</oboInOwl:id>
        <rdfs:label>Governorate of Jizan</rdfs:label>
    </owl:NamedIndividual>
    


    <!-- http://purl.obolibrary.org/obo/GAZ_00031294 -->

    <owl:NamedIndividual rdf:about="http://purl.obolibrary.org/obo/GAZ_00031294">
        <obo:RO_0001025 rdf:resource="http://purl.obolibrary.org/obo/GAZ_00010398"/>
        <oboInOwl:hasOBONamespace>GAZ</oboInOwl:hasOBONamespace>
        <oboInOwl:id>GAZ:00031294</oboInOwl:id>
        <rdfs:label>Governorate of Al-Idabi</rdfs:label>
    </owl:NamedIndividual>
    


    <!-- http://purl.obolibrary.org/obo/GAZ_00031295 -->

    <owl:NamedIndividual rdf:about="http://purl.obolibrary.org/obo/GAZ_00031295">
        <obo:RO_0001025 rdf:resource="http://purl.obolibrary.org/obo/GAZ_00007506"/>
        <oboInOwl:hasOBONamespace>GAZ</oboInOwl:hasOBONamespace>
        <oboInOwl:id>GAZ:00031295</oboInOwl:id>
        <rdfs:label>Governorate of Jiddah</rdfs:label>
    </owl:NamedIndividual>
    


    <!-- http://purl.obolibrary.org/obo/GAZ_00031296 -->

    <owl:NamedIndividual rdf:about="http://purl.obolibrary.org/obo/GAZ_00031296">
        <obo:RO_0001025 rdf:resource="http://purl.obolibrary.org/obo/GAZ_00010398"/>
        <oboInOwl:hasOBONamespace>GAZ</oboInOwl:hasOBONamespace>
        <oboInOwl:id>GAZ:00031296</oboInOwl:id>
        <rdfs:label>Governorate of Samtah</rdfs:label>
    </owl:NamedIndividual>
    


    <!-- http://purl.obolibrary.org/obo/GAZ_00031297 -->

    <owl:NamedIndividual rdf:about="http://purl.obolibrary.org/obo/GAZ_00031297">
        <obo:RO_0001025 rdf:resource="http://purl.obolibrary.org/obo/GAZ_00010398"/>
        <oboInOwl:hasOBONamespace>GAZ</oboInOwl:hasOBONamespace>
        <oboInOwl:id>GAZ:00031297</oboInOwl:id>
        <rdfs:label>Governorate of Ar-Rayth</rdfs:label>
    </owl:NamedIndividual>
    


    <!-- http://purl.obolibrary.org/obo/GAZ_00031298 -->

    <owl:NamedIndividual rdf:about="http://purl.obolibrary.org/obo/GAZ_00031298">
        <obo:RO_0001025 rdf:resource="http://purl.obolibrary.org/obo/GAZ_00007506"/>
        <oboInOwl:hasOBONamespace>GAZ</oboInOwl:hasOBONamespace>
        <oboInOwl:id>GAZ:00031298</oboInOwl:id>
        <rdfs:label>Governorate of Al-Jumum</rdfs:label>
    </owl:NamedIndividual>
    


    <!-- http://purl.obolibrary.org/obo/GAZ_00031299 -->

    <owl:NamedIndividual rdf:about="http://purl.obolibrary.org/obo/GAZ_00031299">
        <obo:RO_0001025 rdf:resource="http://purl.obolibrary.org/obo/GAZ_00007506"/>
        <oboInOwl:hasOBONamespace>GAZ</oboInOwl:hasOBONamespace>
        <oboInOwl:id>GAZ:00031299</oboInOwl:id>
        <rdfs:label>Governorate of Al-Kamil</rdfs:label>
    </owl:NamedIndividual>
    


    <!-- http://purl.obolibrary.org/obo/GAZ_00031300 -->

    <owl:NamedIndividual rdf:about="http://purl.obolibrary.org/obo/GAZ_00031300">
        <obo:RO_0001025 rdf:resource="http://purl.obolibrary.org/obo/GAZ_00007506"/>
        <oboInOwl:hasOBONamespace>GAZ</oboInOwl:hasOBONamespace>
        <oboInOwl:id>GAZ:00031300</oboInOwl:id>
        <rdfs:label>Governorate of Khulays</rdfs:label>
    </owl:NamedIndividual>
    


    <!-- http://purl.obolibrary.org/obo/GAZ_00031301 -->

    <owl:NamedIndividual rdf:about="http://purl.obolibrary.org/obo/GAZ_00031301">
        <obo:RO_0001025 rdf:resource="http://purl.obolibrary.org/obo/GAZ_00007506"/>
        <oboInOwl:hasOBONamespace>GAZ</oboInOwl:hasOBONamespace>
        <oboInOwl:id>GAZ:00031301</oboInOwl:id>
        <rdfs:label>Governorate of Al-Khurmah</rdfs:label>
    </owl:NamedIndividual>
    


    <!-- http://purl.obolibrary.org/obo/GAZ_00031302 -->

    <owl:NamedIndividual rdf:about="http://purl.obolibrary.org/obo/GAZ_00031302">
        <obo:RO_0001025 rdf:resource="http://purl.obolibrary.org/obo/GAZ_00007506"/>
        <oboInOwl:hasOBONamespace>GAZ</oboInOwl:hasOBONamespace>
        <oboInOwl:id>GAZ:00031302</oboInOwl:id>
        <rdfs:label>Governorate of Al-Lith</rdfs:label>
    </owl:NamedIndividual>
    


    <!-- http://purl.obolibrary.org/obo/GAZ_00031303 -->

    <owl:NamedIndividual rdf:about="http://purl.obolibrary.org/obo/GAZ_00031303">
        <obo:RO_0001025 rdf:resource="http://purl.obolibrary.org/obo/GAZ_00007506"/>
        <oboInOwl:hasOBONamespace>GAZ</oboInOwl:hasOBONamespace>
        <oboInOwl:id>GAZ:00031303</oboInOwl:id>
        <rdfs:label>Governorate of Al-Qunfidhah</rdfs:label>
    </owl:NamedIndividual>
    


    <!-- http://purl.obolibrary.org/obo/GAZ_00031304 -->

    <owl:NamedIndividual rdf:about="http://purl.obolibrary.org/obo/GAZ_00031304">
        <obo:RO_0001025 rdf:resource="http://purl.obolibrary.org/obo/GAZ_00007506"/>
        <oboInOwl:hasOBONamespace>GAZ</oboInOwl:hasOBONamespace>
        <oboInOwl:id>GAZ:00031304</oboInOwl:id>
        <rdfs:label>Governorate of Makka</rdfs:label>
    </owl:NamedIndividual>
    


    <!-- http://purl.obolibrary.org/obo/GAZ_00031305 -->

    <owl:NamedIndividual rdf:about="http://purl.obolibrary.org/obo/GAZ_00031305">
        <obo:RO_0001025 rdf:resource="http://purl.obolibrary.org/obo/GAZ_00007506"/>
        <oboInOwl:hasOBONamespace>GAZ</oboInOwl:hasOBONamespace>
        <oboInOwl:id>GAZ:00031305</oboInOwl:id>
        <rdfs:label>Governorate of Rabigh</rdfs:label>
    </owl:NamedIndividual>
    


    <!-- http://purl.obolibrary.org/obo/GAZ_00031306 -->

    <owl:NamedIndividual rdf:about="http://purl.obolibrary.org/obo/GAZ_00031306">
        <obo:RO_0001025 rdf:resource="http://purl.obolibrary.org/obo/GAZ_00007506"/>
        <oboInOwl:hasOBONamespace>GAZ</oboInOwl:hasOBONamespace>
        <oboInOwl:id>GAZ:00031306</oboInOwl:id>
        <rdfs:label>Governorate of Ranyah</rdfs:label>
    </owl:NamedIndividual>
    


    <!-- http://purl.obolibrary.org/obo/GAZ_00031307 -->

    <owl:NamedIndividual rdf:about="http://purl.obolibrary.org/obo/GAZ_00031307">
        <obo:RO_0001025 rdf:resource="http://purl.obolibrary.org/obo/GAZ_00007506"/>
        <oboInOwl:hasOBONamespace>GAZ</oboInOwl:hasOBONamespace>
        <oboInOwl:id>GAZ:00031307</oboInOwl:id>
        <rdfs:label>Governorate of Al-Taif</rdfs:label>
    </owl:NamedIndividual>
    


    <!-- http://purl.obolibrary.org/obo/GAZ_00031308 -->

    <owl:NamedIndividual rdf:about="http://purl.obolibrary.org/obo/GAZ_00031308">
        <obo:RO_0001025 rdf:resource="http://purl.obolibrary.org/obo/GAZ_00007506"/>
        <oboInOwl:hasOBONamespace>GAZ</oboInOwl:hasOBONamespace>
        <oboInOwl:id>GAZ:00031308</oboInOwl:id>
        <rdfs:label>Governorate of Turubah</rdfs:label>
    </owl:NamedIndividual>
    


    <!-- http://purl.obolibrary.org/obo/GAZ_00031309 -->

    <owl:NamedIndividual rdf:about="http://purl.obolibrary.org/obo/GAZ_00031309">
        <obo:RO_0001025 rdf:resource="http://purl.obolibrary.org/obo/GAZ_00015060"/>
        <oboInOwl:hasOBONamespace>GAZ</oboInOwl:hasOBONamespace>
        <oboInOwl:id>GAZ:00031309</oboInOwl:id>
        <rdfs:label>Governorate of Al-Hinakiyah</rdfs:label>
    </owl:NamedIndividual>
    


    <!-- http://purl.obolibrary.org/obo/GAZ_00031310 -->

    <owl:NamedIndividual rdf:about="http://purl.obolibrary.org/obo/GAZ_00031310">
        <obo:RO_0001025 rdf:resource="http://purl.obolibrary.org/obo/GAZ_00015060"/>
        <oboInOwl:hasOBONamespace>GAZ</oboInOwl:hasOBONamespace>
        <oboInOwl:id>GAZ:00031310</oboInOwl:id>
        <rdfs:label>Governorate of Alula</rdfs:label>
    </owl:NamedIndividual>
    


    <!-- http://purl.obolibrary.org/obo/GAZ_00031311 -->

    <owl:NamedIndividual rdf:about="http://purl.obolibrary.org/obo/GAZ_00031311">
        <obo:RO_0001025 rdf:resource="http://purl.obolibrary.org/obo/GAZ_00015060"/>
        <oboInOwl:hasOBONamespace>GAZ</oboInOwl:hasOBONamespace>
        <oboInOwl:id>GAZ:00031311</oboInOwl:id>
        <rdfs:label>Governorate of Khaybar</rdfs:label>
    </owl:NamedIndividual>
    


    <!-- http://purl.obolibrary.org/obo/GAZ_00031312 -->

    <owl:NamedIndividual rdf:about="http://purl.obolibrary.org/obo/GAZ_00031312">
        <obo:RO_0001025 rdf:resource="http://purl.obolibrary.org/obo/GAZ_00015060"/>
        <oboInOwl:hasOBONamespace>GAZ</oboInOwl:hasOBONamespace>
        <oboInOwl:id>GAZ:00031312</oboInOwl:id>
        <rdfs:label>Governorate of Badr</rdfs:label>
    </owl:NamedIndividual>
    


    <!-- http://purl.obolibrary.org/obo/GAZ_00031313 -->

    <owl:NamedIndividual rdf:about="http://purl.obolibrary.org/obo/GAZ_00031313">
        <obo:RO_0001025 rdf:resource="http://purl.obolibrary.org/obo/GAZ_00015060"/>
        <oboInOwl:hasOBONamespace>GAZ</oboInOwl:hasOBONamespace>
        <oboInOwl:id>GAZ:00031313</oboInOwl:id>
        <rdfs:label>Governorate of Al-Madinah</rdfs:label>
    </owl:NamedIndividual>
    


    <!-- http://purl.obolibrary.org/obo/GAZ_00031314 -->

    <owl:NamedIndividual rdf:about="http://purl.obolibrary.org/obo/GAZ_00031314">
        <obo:RO_0001025 rdf:resource="http://purl.obolibrary.org/obo/GAZ_00015060"/>
        <oboInOwl:hasOBONamespace>GAZ</oboInOwl:hasOBONamespace>
        <oboInOwl:id>GAZ:00031314</oboInOwl:id>
        <rdfs:label>Governorate of Al-Mahd</rdfs:label>
    </owl:NamedIndividual>
    


    <!-- http://purl.obolibrary.org/obo/GAZ_00031315 -->

    <owl:NamedIndividual rdf:about="http://purl.obolibrary.org/obo/GAZ_00031315">
        <obo:RO_0001025 rdf:resource="http://purl.obolibrary.org/obo/GAZ_00015060"/>
        <oboInOwl:hasOBONamespace>GAZ</oboInOwl:hasOBONamespace>
        <oboInOwl:id>GAZ:00031315</oboInOwl:id>
        <rdfs:label>Governorate of Yanbu al-Bahr</rdfs:label>
    </owl:NamedIndividual>
    


    <!-- http://purl.obolibrary.org/obo/GAZ_00031316 -->

    <owl:NamedIndividual rdf:about="http://purl.obolibrary.org/obo/GAZ_00031316">
        <obo:RO_0001025 rdf:resource="http://purl.obolibrary.org/obo/GAZ_00015056"/>
        <oboInOwl:hasOBONamespace>GAZ</oboInOwl:hasOBONamespace>
        <oboInOwl:id>GAZ:00031316</oboInOwl:id>
        <rdfs:label>Governorate of Hubuna</rdfs:label>
    </owl:NamedIndividual>
    


    <!-- http://purl.obolibrary.org/obo/GAZ_00031317 -->

    <owl:NamedIndividual rdf:about="http://purl.obolibrary.org/obo/GAZ_00031317">
        <obo:RO_0001025 rdf:resource="http://purl.obolibrary.org/obo/GAZ_00015056"/>
        <oboInOwl:hasOBONamespace>GAZ</oboInOwl:hasOBONamespace>
        <oboInOwl:id>GAZ:00031317</oboInOwl:id>
        <rdfs:label>Governorate of Al-Kharkhir</rdfs:label>
    </owl:NamedIndividual>
    


    <!-- http://purl.obolibrary.org/obo/GAZ_00031318 -->

    <owl:NamedIndividual rdf:about="http://purl.obolibrary.org/obo/GAZ_00031318">
        <obo:RO_0001025 rdf:resource="http://purl.obolibrary.org/obo/GAZ_00015056"/>
        <oboInOwl:hasOBONamespace>GAZ</oboInOwl:hasOBONamespace>
        <oboInOwl:id>GAZ:00031318</oboInOwl:id>
        <rdfs:label>Governorate of Khubash</rdfs:label>
    </owl:NamedIndividual>
    


    <!-- http://purl.obolibrary.org/obo/GAZ_00031319 -->

    <owl:NamedIndividual rdf:about="http://purl.obolibrary.org/obo/GAZ_00031319">
        <obo:RO_0001025 rdf:resource="http://purl.obolibrary.org/obo/GAZ_00015056"/>
        <oboInOwl:hasOBONamespace>GAZ</oboInOwl:hasOBONamespace>
        <oboInOwl:id>GAZ:00031319</oboInOwl:id>
        <rdfs:label>Governorate of Najran</rdfs:label>
    </owl:NamedIndividual>
    


    <!-- http://purl.obolibrary.org/obo/GAZ_00031320 -->

    <owl:NamedIndividual rdf:about="http://purl.obolibrary.org/obo/GAZ_00031320">
        <obo:RO_0001025 rdf:resource="http://purl.obolibrary.org/obo/GAZ_00015056"/>
        <oboInOwl:hasOBONamespace>GAZ</oboInOwl:hasOBONamespace>
        <oboInOwl:id>GAZ:00031320</oboInOwl:id>
        <rdfs:label>Governorate of Sharurah</rdfs:label>
    </owl:NamedIndividual>
    


    <!-- http://purl.obolibrary.org/obo/GAZ_00031321 -->

    <owl:NamedIndividual rdf:about="http://purl.obolibrary.org/obo/GAZ_00031321">
        <obo:RO_0001025 rdf:resource="http://purl.obolibrary.org/obo/GAZ_00015056"/>
        <oboInOwl:hasOBONamespace>GAZ</oboInOwl:hasOBONamespace>
        <oboInOwl:id>GAZ:00031321</oboInOwl:id>
        <rdfs:label>Governorate of Thar</rdfs:label>
    </owl:NamedIndividual>
    


    <!-- http://purl.obolibrary.org/obo/GAZ_00031322 -->

    <owl:NamedIndividual rdf:about="http://purl.obolibrary.org/obo/GAZ_00031322">
        <obo:RO_0001025 rdf:resource="http://purl.obolibrary.org/obo/GAZ_00015056"/>
        <oboInOwl:hasOBONamespace>GAZ</oboInOwl:hasOBONamespace>
        <oboInOwl:id>GAZ:00031322</oboInOwl:id>
        <rdfs:label>Governorate of Yadamah</rdfs:label>
    </owl:NamedIndividual>
    


    <!-- http://purl.obolibrary.org/obo/GAZ_00031323 -->

    <owl:NamedIndividual rdf:about="http://purl.obolibrary.org/obo/GAZ_00031323">
        <obo:RO_0001025 rdf:resource="http://purl.obolibrary.org/obo/GAZ_00015054"/>
        <oboInOwl:hasOBONamespace>GAZ</oboInOwl:hasOBONamespace>
        <oboInOwl:id>GAZ:00031323</oboInOwl:id>
        <rdfs:label>Governorate of Duba</rdfs:label>
    </owl:NamedIndividual>
    


    <!-- http://purl.obolibrary.org/obo/GAZ_00031324 -->

    <owl:NamedIndividual rdf:about="http://purl.obolibrary.org/obo/GAZ_00031324">
        <obo:RO_0001025 rdf:resource="http://purl.obolibrary.org/obo/GAZ_00015054"/>
        <oboInOwl:hasOBONamespace>GAZ</oboInOwl:hasOBONamespace>
        <oboInOwl:id>GAZ:00031324</oboInOwl:id>
        <rdfs:label>Governorate of Haqil</rdfs:label>
    </owl:NamedIndividual>
    


    <!-- http://purl.obolibrary.org/obo/GAZ_00031325 -->

    <owl:NamedIndividual rdf:about="http://purl.obolibrary.org/obo/GAZ_00031325">
        <obo:RO_0001025 rdf:resource="http://purl.obolibrary.org/obo/GAZ_00015054"/>
        <oboInOwl:hasOBONamespace>GAZ</oboInOwl:hasOBONamespace>
        <oboInOwl:id>GAZ:00031325</oboInOwl:id>
        <rdfs:label>Governorate of Tabuk</rdfs:label>
    </owl:NamedIndividual>
    


    <!-- http://purl.obolibrary.org/obo/GAZ_00031326 -->

    <owl:NamedIndividual rdf:about="http://purl.obolibrary.org/obo/GAZ_00031326">
        <obo:RO_0001025 rdf:resource="http://purl.obolibrary.org/obo/GAZ_00015054"/>
        <oboInOwl:hasOBONamespace>GAZ</oboInOwl:hasOBONamespace>
        <oboInOwl:id>GAZ:00031326</oboInOwl:id>
        <rdfs:label>Governorate of Tayma</rdfs:label>
    </owl:NamedIndividual>
    


    <!-- http://purl.obolibrary.org/obo/GAZ_00031327 -->

    <owl:NamedIndividual rdf:about="http://purl.obolibrary.org/obo/GAZ_00031327">
        <obo:RO_0001025 rdf:resource="http://purl.obolibrary.org/obo/GAZ_00015054"/>
        <oboInOwl:hasOBONamespace>GAZ</oboInOwl:hasOBONamespace>
        <oboInOwl:id>GAZ:00031327</oboInOwl:id>
        <rdfs:label>Governorate of Umluj</rdfs:label>
    </owl:NamedIndividual>
    


    <!-- http://purl.obolibrary.org/obo/GAZ_00031328 -->

    <owl:NamedIndividual rdf:about="http://purl.obolibrary.org/obo/GAZ_00031328">
        <obo:RO_0001025 rdf:resource="http://purl.obolibrary.org/obo/GAZ_00015054"/>
        <oboInOwl:hasOBONamespace>GAZ</oboInOwl:hasOBONamespace>
        <oboInOwl:id>GAZ:00031328</oboInOwl:id>
        <rdfs:label>Governorate of Al-Wajh</rdfs:label>
    </owl:NamedIndividual>
    


    <!-- http://purl.obolibrary.org/obo/GAZ_00039902 -->

    <owl:NamedIndividual rdf:about="http://purl.obolibrary.org/obo/GAZ_00039902">
        <obo:RO_0001025 rdf:resource="http://purl.obolibrary.org/obo/GAZ_00102118"/>
        <obo:IAO_0000115>A group of small islands off of the eastern coast of the Horn of Africa, in the Dact-el-Mayun section of the Bab-el-Mandeb strait.</obo:IAO_0000115>
        <oboInOwl:hasOBONamespace>GAZ</oboInOwl:hasOBONamespace>
        <oboInOwl:id>GAZ:00039902</oboInOwl:id>
        <rdfs:label>Sept Freres</rdfs:label>
    </owl:NamedIndividual>
    


    <!-- http://purl.obolibrary.org/obo/GAZ_00039909 -->

    <owl:NamedIndividual rdf:about="http://purl.obolibrary.org/obo/GAZ_00039909">
        <obo:RO_0001025 rdf:resource="http://purl.obolibrary.org/obo/GAZ_00009683"/>
        <obo:IAO_0000115>An island of the Dahlak Archipelago.</obo:IAO_0000115>
        <oboInOwl:hasOBONamespace>GAZ</oboInOwl:hasOBONamespace>
        <oboInOwl:id>GAZ:00039909</oboInOwl:id>
        <rdfs:label>Harmil Island</rdfs:label>
    </owl:NamedIndividual>
    


    <!-- http://purl.obolibrary.org/obo/GAZ_00039910 -->

    <owl:NamedIndividual rdf:about="http://purl.obolibrary.org/obo/GAZ_00039910">
        <obo:RO_0001025 rdf:resource="http://purl.obolibrary.org/obo/GAZ_00009683"/>
        <obo:IAO_0000115>An island of the Dahlak Archipelago.</obo:IAO_0000115>
        <oboInOwl:hasOBONamespace>GAZ</oboInOwl:hasOBONamespace>
        <oboInOwl:id>GAZ:00039910</oboInOwl:id>
        <rdfs:label>Nora Island</rdfs:label>
    </owl:NamedIndividual>
    


    <!-- http://purl.obolibrary.org/obo/GAZ_00039911 -->

    <owl:NamedIndividual rdf:about="http://purl.obolibrary.org/obo/GAZ_00039911">
        <obo:RO_0001025 rdf:resource="http://purl.obolibrary.org/obo/GAZ_00009683"/>
        <obo:IAO_0000115>An island of the Dahlak Archipelago.</obo:IAO_0000115>
        <oboInOwl:hasOBONamespace>GAZ</oboInOwl:hasOBONamespace>
        <oboInOwl:id>GAZ:00039911</oboInOwl:id>
        <rdfs:label>Dahlak Kebir</rdfs:label>
    </owl:NamedIndividual>
    


    <!-- http://purl.obolibrary.org/obo/GAZ_00039912 -->

    <owl:NamedIndividual rdf:about="http://purl.obolibrary.org/obo/GAZ_00039912">
        <obo:RO_0001025 rdf:resource="http://purl.obolibrary.org/obo/GAZ_00009683"/>
        <obo:IAO_0000115>An island of the Dahlak Archipelago.</obo:IAO_0000115>
        <oboInOwl:hasOBONamespace>GAZ</oboInOwl:hasOBONamespace>
        <oboInOwl:id>GAZ:00039912</oboInOwl:id>
        <rdfs:label>Nahaleg Island</rdfs:label>
    </owl:NamedIndividual>
    


    <!-- http://purl.obolibrary.org/obo/GAZ_00039913 -->

    <owl:NamedIndividual rdf:about="http://purl.obolibrary.org/obo/GAZ_00039913">
        <obo:RO_0001025 rdf:resource="http://purl.obolibrary.org/obo/GAZ_00002456"/>
        <obo:IAO_0000115>An island.</obo:IAO_0000115>
        <oboInOwl:hasOBONamespace>GAZ</oboInOwl:hasOBONamespace>
        <oboInOwl:id>GAZ:00039913</oboInOwl:id>
        <rdfs:label>Massawa Island</rdfs:label>
    </owl:NamedIndividual>
    


    <!-- http://purl.obolibrary.org/obo/GAZ_00039915 -->

    <owl:NamedIndividual rdf:about="http://purl.obolibrary.org/obo/GAZ_00039915">
        <obo:RO_0001025 rdf:resource="http://purl.obolibrary.org/obo/GAZ_00248117"/>
        <obo:IAO_0000115>An island.</obo:IAO_0000115>
        <oboInOwl:hasOBONamespace>GAZ</oboInOwl:hasOBONamespace>
        <oboInOwl:id>GAZ:00039915</oboInOwl:id>
        <rdfs:label>Halba Deset</rdfs:label>
    </owl:NamedIndividual>
    


    <!-- http://purl.obolibrary.org/obo/GAZ_00039916 -->

    <owl:NamedIndividual rdf:about="http://purl.obolibrary.org/obo/GAZ_00039916">
        <obo:RO_0001025 rdf:resource="http://purl.obolibrary.org/obo/GAZ_00002456"/>
        <obo:IAO_0000115>Islands.</obo:IAO_0000115>
        <oboInOwl:hasOBONamespace>GAZ</oboInOwl:hasOBONamespace>
        <oboInOwl:id>GAZ:00039916</oboInOwl:id>
        <rdfs:label>Howakil Islands</rdfs:label>
    </owl:NamedIndividual>
    


    <!-- http://purl.obolibrary.org/obo/GAZ_00039917 -->

    <owl:NamedIndividual rdf:about="http://purl.obolibrary.org/obo/GAZ_00039917">
        <obo:RO_0001025 rdf:resource="http://purl.obolibrary.org/obo/GAZ_00009683"/>
        <obo:IAO_0000115>An island of the Dahlak Archipelago.</obo:IAO_0000115>
        <oboInOwl:hasOBONamespace>GAZ</oboInOwl:hasOBONamespace>
        <oboInOwl:id>GAZ:00039917</oboInOwl:id>
        <rdfs:label>Isra-Tu Island</rdfs:label>
    </owl:NamedIndividual>
    


    <!-- http://purl.obolibrary.org/obo/GAZ_00039918 -->

    <owl:NamedIndividual rdf:about="http://purl.obolibrary.org/obo/GAZ_00039918">
        <obo:RO_0001025 rdf:resource="http://purl.obolibrary.org/obo/GAZ_00009683"/>
        <obo:IAO_0000115>An island of the Dahlak Archipelago.</obo:IAO_0000115>
        <oboInOwl:hasOBONamespace>GAZ</oboInOwl:hasOBONamespace>
        <oboInOwl:id>GAZ:00039918</oboInOwl:id>
        <rdfs:label>Shumma Island</rdfs:label>
    </owl:NamedIndividual>
    


    <!-- http://purl.obolibrary.org/obo/GAZ_00039919 -->

    <owl:NamedIndividual rdf:about="http://purl.obolibrary.org/obo/GAZ_00039919">
        <obo:RO_0001025 rdf:resource="http://purl.obolibrary.org/obo/GAZ_00009683"/>
        <obo:IAO_0000115>An island of the Dahlak Archipelago.</obo:IAO_0000115>
        <oboInOwl:hasOBONamespace>GAZ</oboInOwl:hasOBONamespace>
        <oboInOwl:id>GAZ:00039919</oboInOwl:id>
        <rdfs:label>Harat Island</rdfs:label>
    </owl:NamedIndividual>
    


    <!-- http://purl.obolibrary.org/obo/GAZ_00039920 -->

    <owl:NamedIndividual rdf:about="http://purl.obolibrary.org/obo/GAZ_00039920">
        <obo:RO_0001025 rdf:resource="http://purl.obolibrary.org/obo/GAZ_00009683"/>
        <obo:IAO_0000115>An island of the Dahlak Archipelago.</obo:IAO_0000115>
        <oboInOwl:hasOBONamespace>GAZ</oboInOwl:hasOBONamespace>
        <oboInOwl:id>GAZ:00039920</oboInOwl:id>
        <rdfs:label>Dissei Island</rdfs:label>
    </owl:NamedIndividual>
    


    <!-- http://purl.obolibrary.org/obo/GAZ_00039921 -->

    <owl:NamedIndividual rdf:about="http://purl.obolibrary.org/obo/GAZ_00039921">
        <obo:RO_0001025 rdf:resource="http://purl.obolibrary.org/obo/GAZ_00009683"/>
        <obo:IAO_0000115>An island of the Dahlak Archipelago.</obo:IAO_0000115>
        <oboInOwl:hasOBONamespace>GAZ</oboInOwl:hasOBONamespace>
        <oboInOwl:id>GAZ:00039921</oboInOwl:id>
        <rdfs:label>Erwa Island</rdfs:label>
    </owl:NamedIndividual>
    


    <!-- http://purl.obolibrary.org/obo/GAZ_00039922 -->

    <owl:NamedIndividual rdf:about="http://purl.obolibrary.org/obo/GAZ_00039922">
        <obo:RO_0001025 rdf:resource="http://purl.obolibrary.org/obo/GAZ_00009683"/>
        <obo:IAO_0000115>An island of the Dahlak Archipelago.</obo:IAO_0000115>
        <oboInOwl:hasOBONamespace>GAZ</oboInOwl:hasOBONamespace>
        <oboInOwl:id>GAZ:00039922</oboInOwl:id>
        <rdfs:label>Dohul Island</rdfs:label>
    </owl:NamedIndividual>
    


    <!-- http://purl.obolibrary.org/obo/GAZ_00039923 -->

    <owl:NamedIndividual rdf:about="http://purl.obolibrary.org/obo/GAZ_00039923">
        <obo:RO_0001025 rdf:resource="http://purl.obolibrary.org/obo/GAZ_00009683"/>
        <obo:IAO_0000115>An island of the Dahlak Archipelago.</obo:IAO_0000115>
        <oboInOwl:hasOBONamespace>GAZ</oboInOwl:hasOBONamespace>
        <oboInOwl:id>GAZ:00039923</oboInOwl:id>
        <rdfs:label>Dhuladhiya Island</rdfs:label>
    </owl:NamedIndividual>
    


    <!-- http://purl.obolibrary.org/obo/GAZ_00045691 -->

    <owl:NamedIndividual rdf:about="http://purl.obolibrary.org/obo/GAZ_00045691">
        <obo:RO_0001025 rdf:resource="http://purl.obolibrary.org/obo/GAZ_00018525"/>
        <obo:IAO_0000115>An island.</obo:IAO_0000115>
        <oboInOwl:hasOBONamespace>GAZ</oboInOwl:hasOBONamespace>
        <oboInOwl:id>GAZ:00045691</oboInOwl:id>
        <rdfs:label>Greater Tunb</rdfs:label>
    </owl:NamedIndividual>
    


    <!-- http://purl.obolibrary.org/obo/GAZ_00045692 -->

    <owl:NamedIndividual rdf:about="http://purl.obolibrary.org/obo/GAZ_00045692">
        <obo:RO_0001025 rdf:resource="http://purl.obolibrary.org/obo/GAZ_00018525"/>
        <obo:IAO_0000115>An island.</obo:IAO_0000115>
        <oboInOwl:hasOBONamespace>GAZ</oboInOwl:hasOBONamespace>
        <oboInOwl:id>GAZ:00045692</oboInOwl:id>
        <rdfs:label>Lesser Tunb</rdfs:label>
    </owl:NamedIndividual>
    


    <!-- http://purl.obolibrary.org/obo/GAZ_00047079 -->

    <owl:NamedIndividual rdf:about="http://purl.obolibrary.org/obo/GAZ_00047079">
        <obo:RO_0001025 rdf:resource="http://purl.obolibrary.org/obo/GAZ_00005295"/>
        <obo:IAO_0000115>An offshore Island in the Persian Gulf.</obo:IAO_0000115>
        <oboInOwl:hasOBONamespace>GAZ</oboInOwl:hasOBONamespace>
        <oboInOwl:id>GAZ:00047079</oboInOwl:id>
        <rdfs:label>Das</rdfs:label>
    </owl:NamedIndividual>
    


    <!-- http://purl.obolibrary.org/obo/GAZ_00047080 -->

    <owl:NamedIndividual rdf:about="http://purl.obolibrary.org/obo/GAZ_00047080">
        <obo:RO_0001025 rdf:resource="http://purl.obolibrary.org/obo/GAZ_00005295"/>
        <obo:IAO_0000115>An island off the coast of Abu Dhabi, United Arab Emirates.</obo:IAO_0000115>
        <oboInOwl:hasOBONamespace>GAZ</oboInOwl:hasOBONamespace>
        <oboInOwl:id>GAZ:00047080</oboInOwl:id>
        <rdfs:label>Dalma Island</rdfs:label>
    </owl:NamedIndividual>
    


    <!-- http://purl.obolibrary.org/obo/GAZ_00047081 -->

    <owl:NamedIndividual rdf:about="http://purl.obolibrary.org/obo/GAZ_00047081">
        <obo:RO_0001025 rdf:resource="http://purl.obolibrary.org/obo/GAZ_00005295"/>
        <obo:IAO_0000115>An island.</obo:IAO_0000115>
        <oboInOwl:hasOBONamespace>GAZ</oboInOwl:hasOBONamespace>
        <oboInOwl:id>GAZ:00047081</oboInOwl:id>
        <rdfs:label>Arzanah Island</rdfs:label>
    </owl:NamedIndividual>
    


    <!-- http://purl.obolibrary.org/obo/GAZ_00048421 -->

    <owl:NamedIndividual rdf:about="http://purl.obolibrary.org/obo/GAZ_00048421">
        <obo:RO_0001025 rdf:resource="http://purl.obolibrary.org/obo/GAZ_00006936"/>
        <oboInOwl:hasOBONamespace>GAZ</oboInOwl:hasOBONamespace>
        <oboInOwl:id>GAZ:00048421</oboInOwl:id>
        <rdfs:label>Al Hidd Island</rdfs:label>
    </owl:NamedIndividual>
    


    <!-- http://purl.obolibrary.org/obo/GAZ_00048570 -->

    <owl:NamedIndividual rdf:about="http://purl.obolibrary.org/obo/GAZ_00048570">
        <obo:RO_0001025 rdf:resource="http://purl.obolibrary.org/obo/GAZ_00002456"/>
        <oboInOwl:hasOBONamespace>GAZ</oboInOwl:hasOBONamespace>
        <oboInOwl:id>GAZ:00048570</oboInOwl:id>
        <rdfs:label>Gifatin Island</rdfs:label>
    </owl:NamedIndividual>
    


    <!-- http://purl.obolibrary.org/obo/GAZ_00048571 -->

    <owl:NamedIndividual rdf:about="http://purl.obolibrary.org/obo/GAZ_00048571">
        <obo:RO_0001025 rdf:resource="http://purl.obolibrary.org/obo/GAZ_00002456"/>
        <oboInOwl:hasOBONamespace>GAZ</oboInOwl:hasOBONamespace>
        <oboInOwl:id>GAZ:00048571</oboInOwl:id>
        <rdfs:label>Qeisum Island</rdfs:label>
    </owl:NamedIndividual>
    


    <!-- http://purl.obolibrary.org/obo/GAZ_00048572 -->

    <owl:NamedIndividual rdf:about="http://purl.obolibrary.org/obo/GAZ_00048572">
        <obo:RO_0001025 rdf:resource="http://purl.obolibrary.org/obo/GAZ_00002456"/>
        <obo:IAO_0000115>An island in the Red Sea.</obo:IAO_0000115>
        <oboInOwl:hasOBONamespace>GAZ</oboInOwl:hasOBONamespace>
        <oboInOwl:id>GAZ:00048572</oboInOwl:id>
        <rdfs:label>Tawila Island</rdfs:label>
    </owl:NamedIndividual>
    


    <!-- http://purl.obolibrary.org/obo/GAZ_00048573 -->

    <owl:NamedIndividual rdf:about="http://purl.obolibrary.org/obo/GAZ_00048573">
        <obo:RO_0001025 rdf:resource="http://purl.obolibrary.org/obo/GAZ_00002456"/>
        <oboInOwl:hasOBONamespace>GAZ</oboInOwl:hasOBONamespace>
        <oboInOwl:id>GAZ:00048573</oboInOwl:id>
        <rdfs:label>Gubal Island</rdfs:label>
    </owl:NamedIndividual>
    


    <!-- http://purl.obolibrary.org/obo/GAZ_00049003 -->

    <owl:NamedIndividual rdf:about="http://purl.obolibrary.org/obo/GAZ_00049003">
        <obo:RO_0001025 rdf:resource="http://purl.obolibrary.org/obo/GAZ_00002456"/>
        <obo:RO_0001025 rdf:resource="http://purl.obolibrary.org/obo/GAZ_00010398"/>
        <obo:IAO_0000115>A large coral island group in the Red Sea, belonging to Saudi Arabia. It is located some 40 km offshore from Jizan, in the far southwestern part of the country.</obo:IAO_0000115>
        <oboInOwl:hasOBONamespace>GAZ</oboInOwl:hasOBONamespace>
        <oboInOwl:id>GAZ:00049003</oboInOwl:id>
        <rdfs:label>Farasan Islands</rdfs:label>
    </owl:NamedIndividual>
    


    <!-- http://purl.obolibrary.org/obo/GAZ_00049004 -->

    <owl:NamedIndividual rdf:about="http://purl.obolibrary.org/obo/GAZ_00049004">
        <obo:RO_0001025 rdf:resource="http://purl.obolibrary.org/obo/GAZ_00049003"/>
        <obo:IAO_0000115>One of the Farasan Islands in Saudi Arabia.</obo:IAO_0000115>
        <oboInOwl:hasOBONamespace>GAZ</oboInOwl:hasOBONamespace>
        <oboInOwl:id>GAZ:00049004</oboInOwl:id>
        <rdfs:label>Zufaf Island</rdfs:label>
    </owl:NamedIndividual>
    


    <!-- http://purl.obolibrary.org/obo/GAZ_00049005 -->

    <owl:NamedIndividual rdf:about="http://purl.obolibrary.org/obo/GAZ_00049005">
        <obo:RO_0001025 rdf:resource="http://purl.obolibrary.org/obo/GAZ_00049003"/>
        <obo:IAO_0000115>One of the Farasan Islands in Saudi Arabia.</obo:IAO_0000115>
        <oboInOwl:hasOBONamespace>GAZ</oboInOwl:hasOBONamespace>
        <oboInOwl:id>GAZ:00049005</oboInOwl:id>
        <rdfs:label>Sajid Island</rdfs:label>
    </owl:NamedIndividual>
    


    <!-- http://purl.obolibrary.org/obo/GAZ_00049006 -->

    <owl:NamedIndividual rdf:about="http://purl.obolibrary.org/obo/GAZ_00049006">
        <obo:RO_0001025 rdf:resource="http://purl.obolibrary.org/obo/GAZ_00049003"/>
        <obo:IAO_0000115>The largest island of the Farasan Islands, in the Red Sea. It is located some 50 km offshore from Jizan, the far southwestern part of Saudi Arabia.</obo:IAO_0000115>
        <oboInOwl:hasOBONamespace>GAZ</oboInOwl:hasOBONamespace>
        <oboInOwl:id>GAZ:00049006</oboInOwl:id>
        <rdfs:label>Farasan Island</rdfs:label>
    </owl:NamedIndividual>
    


    <!-- http://purl.obolibrary.org/obo/GAZ_00049007 -->

    <owl:NamedIndividual rdf:about="http://purl.obolibrary.org/obo/GAZ_00049007">
        <obo:RO_0001025 rdf:resource="http://purl.obolibrary.org/obo/GAZ_00007862"/>
        <obo:IAO_0000115>The narrow sea passages, about 13 km wide, between the Sinai and Arabian peninsulas which separates the Gulf of Aqaba from the Red Sea.</obo:IAO_0000115>
        <oboInOwl:hasOBONamespace>GAZ</oboInOwl:hasOBONamespace>
        <oboInOwl:id>GAZ:00049007</oboInOwl:id>
        <rdfs:label>Straits of Tiran</rdfs:label>
    </owl:NamedIndividual>
    


    <!-- http://purl.obolibrary.org/obo/GAZ_00049008 -->

    <owl:NamedIndividual rdf:about="http://purl.obolibrary.org/obo/GAZ_00049008">
        <obo:RO_0001025 rdf:resource="http://purl.obolibrary.org/obo/GAZ_00015054"/>
        <obo:RO_0001025 rdf:resource="http://purl.obolibrary.org/obo/GAZ_00049007"/>
        <obo:IAO_0000115>A Saudi Arabian island in the Straits of Tiran east of Tiran Island.</obo:IAO_0000115>
        <oboInOwl:hasOBONamespace>GAZ</oboInOwl:hasOBONamespace>
        <oboInOwl:id>GAZ:00049008</oboInOwl:id>
        <rdfs:label>Sanafir Island</rdfs:label>
    </owl:NamedIndividual>
    


    <!-- http://purl.obolibrary.org/obo/GAZ_00049009 -->

    <owl:NamedIndividual rdf:about="http://purl.obolibrary.org/obo/GAZ_00049009">
        <obo:RO_0001025 rdf:resource="http://purl.obolibrary.org/obo/GAZ_00015054"/>
        <obo:RO_0001025 rdf:resource="http://purl.obolibrary.org/obo/GAZ_00049007"/>
        <obo:IAO_0000115>An island belonging to Saudi Arabia at the entrance of the Straits of Tiran, which separates the Red Sea and the Gulf of Aqaba.</obo:IAO_0000115>
        <oboInOwl:hasOBONamespace>GAZ</oboInOwl:hasOBONamespace>
        <oboInOwl:id>GAZ:00049009</oboInOwl:id>
        <rdfs:label>Tiran Island</rdfs:label>
    </owl:NamedIndividual>
    


    <!-- http://purl.obolibrary.org/obo/GAZ_00049020 -->

    <owl:NamedIndividual rdf:about="http://purl.obolibrary.org/obo/GAZ_00049020">
        <obo:RO_0001025 rdf:resource="http://purl.obolibrary.org/obo/GAZ_00005295"/>
        <obo:IAO_0000115>The largest of about 200 islands along the coast of the United Arab Emirates. It is situated in the emirate of Abu Dhabi.</obo:IAO_0000115>
        <oboInOwl:hasOBONamespace>GAZ</oboInOwl:hasOBONamespace>
        <oboInOwl:id>GAZ:00049020</oboInOwl:id>
        <rdfs:label>Abu al Abyad</rdfs:label>
    </owl:NamedIndividual>
    


    <!-- http://purl.obolibrary.org/obo/GAZ_00049021 -->

    <owl:NamedIndividual rdf:about="http://purl.obolibrary.org/obo/GAZ_00049021">
        <obo:RO_0001025 rdf:resource="http://purl.obolibrary.org/obo/GAZ_00002456"/>
        <obo:IAO_0000115>An island in the Red Sea.</obo:IAO_0000115>
        <oboInOwl:hasOBONamespace>GAZ</oboInOwl:hasOBONamespace>
        <oboInOwl:id>GAZ:00049021</oboInOwl:id>
        <rdfs:label>Jazirat Antufish</rdfs:label>
    </owl:NamedIndividual>
    


    <!-- http://purl.obolibrary.org/obo/GAZ_00051094 -->

    <owl:NamedIndividual rdf:about="http://purl.obolibrary.org/obo/GAZ_00051094">
        <obo:RO_0001025 rdf:resource="http://purl.obolibrary.org/obo/GAZ_00002456"/>
        <oboInOwl:hasOBONamespace>GAZ</oboInOwl:hasOBONamespace>
        <oboInOwl:id>GAZ:00051094</oboInOwl:id>
        <rdfs:label>Strait of Gubal</rdfs:label>
    </owl:NamedIndividual>
    


    <!-- http://purl.obolibrary.org/obo/GAZ_00051269 -->

    <owl:NamedIndividual rdf:about="http://purl.obolibrary.org/obo/GAZ_00051269">
        <obo:RO_0001025 rdf:resource="http://purl.obolibrary.org/obo/GAZ_00002456"/>
        <obo:IAO_0000115>A strait connecting the Red Sea to the Indian Ocean in the Gulf of Aden. The Yemeni island of Perim divides the strait into two channels.</obo:IAO_0000115>
        <oboInOwl:hasOBONamespace>GAZ</oboInOwl:hasOBONamespace>
        <oboInOwl:id>GAZ:00051269</oboInOwl:id>
        <rdfs:label>Bab-el-Mandeb</rdfs:label>
    </owl:NamedIndividual>
    


    <!-- http://purl.obolibrary.org/obo/GAZ_00053592 -->

    <owl:NamedIndividual rdf:about="http://purl.obolibrary.org/obo/GAZ_00053592">
        <obo:RO_0001025 rdf:resource="http://purl.obolibrary.org/obo/GAZ_00002456"/>
        <obo:IAO_0000115>A stratovolcano rises from a 1200 m depth in the south-central Red Sea, forming an oval-shaped island about 3 km long. Located northwest of the constricted Bab al-Mandab passage at the mouth of the Red Sea, about half way between Yemen and Eritrea.</obo:IAO_0000115>
        <oboInOwl:hasOBONamespace>GAZ</oboInOwl:hasOBONamespace>
        <oboInOwl:id>GAZ:00053592</oboInOwl:id>
        <rdfs:label>Jabal al-Tair Island</rdfs:label>
    </owl:NamedIndividual>
    


    <!-- http://purl.obolibrary.org/obo/GAZ_00053593 -->

    <owl:NamedIndividual rdf:about="http://purl.obolibrary.org/obo/GAZ_00053593">
        <obo:RO_0001025 rdf:resource="http://purl.obolibrary.org/obo/GAZ_00053592"/>
        <obo:IAO_0000115>A volcanic vent.</obo:IAO_0000115>
        <oboInOwl:hasOBONamespace>GAZ</oboInOwl:hasOBONamespace>
        <oboInOwl:id>GAZ:00053593</oboInOwl:id>
        <rdfs:label>Jebel Duchan</rdfs:label>
    </owl:NamedIndividual>
    


    <!-- http://purl.obolibrary.org/obo/GAZ_00053594 -->

    <owl:NamedIndividual rdf:about="http://purl.obolibrary.org/obo/GAZ_00053594">
        <obo:RO_0001025 rdf:resource="http://purl.obolibrary.org/obo/GAZ_00002456"/>
        <obo:IAO_0000115>The largest of a group of 10 small islands and submerged shoals that rise from a shallow platform in the Red Sea rift.</obo:IAO_0000115>
        <oboInOwl:hasOBONamespace>GAZ</oboInOwl:hasOBONamespace>
        <oboInOwl:id>GAZ:00053594</oboInOwl:id>
        <rdfs:label>Jebel Zubair</rdfs:label>
    </owl:NamedIndividual>
    


    <!-- http://purl.obolibrary.org/obo/GAZ_00053595 -->

    <owl:NamedIndividual rdf:about="http://purl.obolibrary.org/obo/GAZ_00053595">
        <obo:RO_0001025 rdf:resource="http://purl.obolibrary.org/obo/GAZ_00005876"/>
        <obo:IAO_0000115>The largest of the Hanish Islands, which belong to Yemen.</obo:IAO_0000115>
        <oboInOwl:hasOBONamespace>GAZ</oboInOwl:hasOBONamespace>
        <oboInOwl:id>GAZ:00053595</oboInOwl:id>
        <rdfs:label>Great Hanish Island</rdfs:label>
    </owl:NamedIndividual>
    


    <!-- http://purl.obolibrary.org/obo/GAZ_00053596 -->

    <owl:NamedIndividual rdf:about="http://purl.obolibrary.org/obo/GAZ_00053596">
        <obo:RO_0001025 rdf:resource="http://purl.obolibrary.org/obo/GAZ_00005876"/>
        <oboInOwl:hasOBONamespace>GAZ</oboInOwl:hasOBONamespace>
        <oboInOwl:id>GAZ:00053596</oboInOwl:id>
        <rdfs:label>Little Hanish Island</rdfs:label>
    </owl:NamedIndividual>
    


    <!-- http://purl.obolibrary.org/obo/GAZ_00053597 -->

    <owl:NamedIndividual rdf:about="http://purl.obolibrary.org/obo/GAZ_00053597">
        <obo:RO_0001025 rdf:resource="http://purl.obolibrary.org/obo/GAZ_00002456"/>
        <oboInOwl:hasOBONamespace>GAZ</oboInOwl:hasOBONamespace>
        <oboInOwl:id>GAZ:00053597</oboInOwl:id>
        <rdfs:label>Zukur-Hanish island group</rdfs:label>
    </owl:NamedIndividual>
    


    <!-- http://purl.obolibrary.org/obo/GAZ_00053683 -->

    <owl:NamedIndividual rdf:about="http://purl.obolibrary.org/obo/GAZ_00053683">
        <obo:IAO_0000115>A volcanic field in the Anti-Lebanon Mountains of SW Syria near the borders with Lebanon and Israel contains numerous cinder cones of Pliocene-to-Holocene age. The Golan Heights volcanic field covers a broad area NE of the Lake Tiberius (the Sea of Galilee) and SW of the city of Damascus (Dimashq) and includes the prehistoric cone of Majdel Shams in the Golan Heights. The volcanic field lies on a basaltic plateau that dips to the west and SW, with steep slopes facing the Dead Sea rift valley. It lies within the northern part of the massive alkaline Harrat Ash Shaam volcanic field that extends from southern Syria through NW Jordan to Saudi Arabia.</obo:IAO_0000115>
        <oboInOwl:hasOBONamespace>GAZ</oboInOwl:hasOBONamespace>
        <oboInOwl:id>GAZ:00053683</oboInOwl:id>
        <rdfs:label>Golan Heights Volcanic Field</rdfs:label>
    </owl:NamedIndividual>
    


    <!-- http://purl.obolibrary.org/obo/GAZ_00053684 -->

    <owl:NamedIndividual rdf:about="http://purl.obolibrary.org/obo/GAZ_00053684">
        <obo:IAO_0000115>A volcanic field, in southern Syria SE of the capital city of Damascas (Dimashq), consists of a lava field with broad areas containing Holocene volcanic vents. The basaltic field contains numerous vents erupted from NW-SE-trending fissures. A boiling lava lake was observed in the Es Safa volcanic area in the middle of the 19th century. This volcanic field lies within the northern part of the massive alkaline Harrat Ash Shaam volcanic field that extends from southern Syria through NE Jordan to Saudi Arabia.</obo:IAO_0000115>
        <oboInOwl:hasOBONamespace>GAZ</oboInOwl:hasOBONamespace>
        <oboInOwl:id>GAZ:00053684</oboInOwl:id>
        <rdfs:label>Es Safa Volcanic Field</rdfs:label>
    </owl:NamedIndividual>
    


    <!-- http://purl.obolibrary.org/obo/GAZ_00053685 -->

    <owl:NamedIndividual rdf:about="http://purl.obolibrary.org/obo/GAZ_00053685">
        <obo:IAO_0000115>A lava region in southern Syria. It lies about 65 km east of Damascus, located in the central part of the administrative district of Muhafazat Rif Dimashq.</obo:IAO_0000115>
        <oboInOwl:hasOBONamespace>GAZ</oboInOwl:hasOBONamespace>
        <oboInOwl:id>GAZ:00053685</oboInOwl:id>
        <rdfs:label>Dirat at Tulul</rdfs:label>
    </owl:NamedIndividual>
    


    <!-- http://purl.obolibrary.org/obo/GAZ_00053686 -->

    <owl:NamedIndividual rdf:about="http://purl.obolibrary.org/obo/GAZ_00053686">
        <obo:RO_0001025 rdf:resource="http://purl.obolibrary.org/obo/GAZ_00014012"/>
        <obo:IAO_0000115>The most prominent feature of Jabal ad Druze Volcanic Field.</obo:IAO_0000115>
        <oboInOwl:hasOBONamespace>GAZ</oboInOwl:hasOBONamespace>
        <oboInOwl:id>GAZ:00053686</oboInOwl:id>
        <rdfs:label>Jabal ad Druze Volcano</rdfs:label>
    </owl:NamedIndividual>
    


    <!-- http://purl.obolibrary.org/obo/GAZ_00053688 -->

    <owl:NamedIndividual rdf:about="http://purl.obolibrary.org/obo/GAZ_00053688">
        <obo:RO_0001025 rdf:resource="http://purl.obolibrary.org/obo/GAZ_00053685"/>
        <obo:IAO_0000115>A volcanic cone.</obo:IAO_0000115>
        <oboInOwl:hasOBONamespace>GAZ</oboInOwl:hasOBONamespace>
        <oboInOwl:id>GAZ:00053688</oboInOwl:id>
        <rdfs:label>Tell Um el Meza</rdfs:label>
    </owl:NamedIndividual>
    


    <!-- http://purl.obolibrary.org/obo/GAZ_00053689 -->

    <owl:NamedIndividual rdf:about="http://purl.obolibrary.org/obo/GAZ_00053689">
        <obo:RO_0001025 rdf:resource="http://purl.obolibrary.org/obo/GAZ_00053685"/>
        <obo:IAO_0000115>A volcanic cone.</obo:IAO_0000115>
        <oboInOwl:hasOBONamespace>GAZ</oboInOwl:hasOBONamespace>
        <oboInOwl:id>GAZ:00053689</oboInOwl:id>
        <rdfs:label>Tell Salman</rdfs:label>
    </owl:NamedIndividual>
    


    <!-- http://purl.obolibrary.org/obo/GAZ_00053690 -->

    <owl:NamedIndividual rdf:about="http://purl.obolibrary.org/obo/GAZ_00053690">
        <obo:RO_0001025 rdf:resource="http://purl.obolibrary.org/obo/GAZ_00053685"/>
        <obo:IAO_0000115>A volcanic cone.</obo:IAO_0000115>
        <oboInOwl:hasOBONamespace>GAZ</oboInOwl:hasOBONamespace>
        <oboInOwl:id>GAZ:00053690</oboInOwl:id>
        <rdfs:label>Tell Aajer</rdfs:label>
    </owl:NamedIndividual>
    


    <!-- http://purl.obolibrary.org/obo/GAZ_00053691 -->

    <owl:NamedIndividual rdf:about="http://purl.obolibrary.org/obo/GAZ_00053691">
        <obo:RO_0001025 rdf:resource="http://purl.obolibrary.org/obo/GAZ_00053685"/>
        <obo:IAO_0000115>A volcanic cone.</obo:IAO_0000115>
        <oboInOwl:hasOBONamespace>GAZ</oboInOwl:hasOBONamespace>
        <oboInOwl:id>GAZ:00053691</oboInOwl:id>
        <rdfs:label>Tell Maqhool</rdfs:label>
    </owl:NamedIndividual>
    


    <!-- http://purl.obolibrary.org/obo/GAZ_00053692 -->

    <owl:NamedIndividual rdf:about="http://purl.obolibrary.org/obo/GAZ_00053692">
        <obo:RO_0001025 rdf:resource="http://purl.obolibrary.org/obo/GAZ_00053685"/>
        <obo:IAO_0000115>A volcanic cone.</obo:IAO_0000115>
        <oboInOwl:hasOBONamespace>GAZ</oboInOwl:hasOBONamespace>
        <oboInOwl:id>GAZ:00053692</oboInOwl:id>
        <rdfs:label>Tell Daqwa</rdfs:label>
    </owl:NamedIndividual>
    


    <!-- http://purl.obolibrary.org/obo/GAZ_00053693 -->

    <owl:NamedIndividual rdf:about="http://purl.obolibrary.org/obo/GAZ_00053693">
        <obo:RO_0001025 rdf:resource="http://purl.obolibrary.org/obo/GAZ_00053685"/>
        <obo:IAO_0000115>A volcanic cone.</obo:IAO_0000115>
        <oboInOwl:hasOBONamespace>GAZ</oboInOwl:hasOBONamespace>
        <oboInOwl:id>GAZ:00053693</oboInOwl:id>
        <rdfs:label>Tell Um Masarja</rdfs:label>
    </owl:NamedIndividual>
    


    <!-- http://purl.obolibrary.org/obo/GAZ_00053694 -->

    <owl:NamedIndividual rdf:about="http://purl.obolibrary.org/obo/GAZ_00053694">
        <obo:RO_0001025 rdf:resource="http://purl.obolibrary.org/obo/GAZ_00053685"/>
        <obo:IAO_0000115>A volcanic cone.</obo:IAO_0000115>
        <oboInOwl:hasOBONamespace>GAZ</oboInOwl:hasOBONamespace>
        <oboInOwl:id>GAZ:00053694</oboInOwl:id>
        <rdfs:label>Tell El Matalla</rdfs:label>
    </owl:NamedIndividual>
    


    <!-- http://purl.obolibrary.org/obo/GAZ_00053695 -->

    <owl:NamedIndividual rdf:about="http://purl.obolibrary.org/obo/GAZ_00053695">
        <obo:RO_0001025 rdf:resource="http://purl.obolibrary.org/obo/GAZ_00053685"/>
        <obo:IAO_0000115>A volcanic cone.</obo:IAO_0000115>
        <oboInOwl:hasOBONamespace>GAZ</oboInOwl:hasOBONamespace>
        <oboInOwl:id>GAZ:00053695</oboInOwl:id>
        <rdfs:label>Tell Wastani</rdfs:label>
    </owl:NamedIndividual>
    


    <!-- http://purl.obolibrary.org/obo/GAZ_00053696 -->

    <owl:NamedIndividual rdf:about="http://purl.obolibrary.org/obo/GAZ_00053696">
        <obo:RO_0001025 rdf:resource="http://purl.obolibrary.org/obo/GAZ_00053685"/>
        <obo:IAO_0000115>A volcanic cone.</obo:IAO_0000115>
        <oboInOwl:hasOBONamespace>GAZ</oboInOwl:hasOBONamespace>
        <oboInOwl:id>GAZ:00053696</oboInOwl:id>
        <rdfs:label>Tell Um Otek</rdfs:label>
    </owl:NamedIndividual>
    


    <!-- http://purl.obolibrary.org/obo/GAZ_00053697 -->

    <owl:NamedIndividual rdf:about="http://purl.obolibrary.org/obo/GAZ_00053697">
        <obo:RO_0001025 rdf:resource="http://purl.obolibrary.org/obo/GAZ_00053685"/>
        <obo:IAO_0000115>A volcanic cone.</obo:IAO_0000115>
        <oboInOwl:hasOBONamespace>GAZ</oboInOwl:hasOBONamespace>
        <oboInOwl:id>GAZ:00053697</oboInOwl:id>
        <rdfs:label>Tell Abu Safa</rdfs:label>
    </owl:NamedIndividual>
    


    <!-- http://purl.obolibrary.org/obo/GAZ_00053698 -->

    <owl:NamedIndividual rdf:about="http://purl.obolibrary.org/obo/GAZ_00053698">
        <obo:RO_0001025 rdf:resource="http://purl.obolibrary.org/obo/GAZ_00053685"/>
        <obo:IAO_0000115>A volcanic cone.</obo:IAO_0000115>
        <oboInOwl:hasOBONamespace>GAZ</oboInOwl:hasOBONamespace>
        <oboInOwl:id>GAZ:00053698</oboInOwl:id>
        <rdfs:label>Tell Jaafar</rdfs:label>
    </owl:NamedIndividual>
    


    <!-- http://purl.obolibrary.org/obo/GAZ_00053699 -->

    <owl:NamedIndividual rdf:about="http://purl.obolibrary.org/obo/GAZ_00053699">
        <obo:RO_0001025 rdf:resource="http://purl.obolibrary.org/obo/GAZ_00053685"/>
        <obo:IAO_0000115>A volcanic cone.</obo:IAO_0000115>
        <oboInOwl:hasOBONamespace>GAZ</oboInOwl:hasOBONamespace>
        <oboInOwl:id>GAZ:00053699</oboInOwl:id>
        <rdfs:label>Tell Shayaba</rdfs:label>
    </owl:NamedIndividual>
    


    <!-- http://purl.obolibrary.org/obo/GAZ_00053700 -->

    <owl:NamedIndividual rdf:about="http://purl.obolibrary.org/obo/GAZ_00053700">
        <obo:RO_0001025 rdf:resource="http://purl.obolibrary.org/obo/GAZ_00053685"/>
        <obo:IAO_0000115>A volcanic cone.</obo:IAO_0000115>
        <oboInOwl:hasOBONamespace>GAZ</oboInOwl:hasOBONamespace>
        <oboInOwl:id>GAZ:00053700</oboInOwl:id>
        <rdfs:label>Tell Khneifes</rdfs:label>
    </owl:NamedIndividual>
    


    <!-- http://purl.obolibrary.org/obo/GAZ_00053701 -->

    <owl:NamedIndividual rdf:about="http://purl.obolibrary.org/obo/GAZ_00053701">
        <obo:RO_0001025 rdf:resource="http://purl.obolibrary.org/obo/GAZ_00053685"/>
        <obo:IAO_0000115>A volcanic cone.</obo:IAO_0000115>
        <oboInOwl:hasOBONamespace>GAZ</oboInOwl:hasOBONamespace>
        <oboInOwl:id>GAZ:00053701</oboInOwl:id>
        <rdfs:label>Tell Hweijer</rdfs:label>
    </owl:NamedIndividual>
    


    <!-- http://purl.obolibrary.org/obo/GAZ_00053702 -->

    <owl:NamedIndividual rdf:about="http://purl.obolibrary.org/obo/GAZ_00053702">
        <obo:RO_0001025 rdf:resource="http://purl.obolibrary.org/obo/GAZ_00053685"/>
        <obo:IAO_0000115>A volcanic cone.</obo:IAO_0000115>
        <oboInOwl:hasOBONamespace>GAZ</oboInOwl:hasOBONamespace>
        <oboInOwl:id>GAZ:00053702</oboInOwl:id>
        <rdfs:label>Tell Shimali</rdfs:label>
    </owl:NamedIndividual>
    


    <!-- http://purl.obolibrary.org/obo/GAZ_00053703 -->

    <owl:NamedIndividual rdf:about="http://purl.obolibrary.org/obo/GAZ_00053703">
        <obo:RO_0001025 rdf:resource="http://purl.obolibrary.org/obo/GAZ_00053685"/>
        <obo:IAO_0000115>A volcanic cone.</obo:IAO_0000115>
        <oboInOwl:hasOBONamespace>GAZ</oboInOwl:hasOBONamespace>
        <oboInOwl:id>GAZ:00053703</oboInOwl:id>
        <rdfs:label>Tell Hweimel</rdfs:label>
    </owl:NamedIndividual>
    


    <!-- http://purl.obolibrary.org/obo/GAZ_00053704 -->

    <owl:NamedIndividual rdf:about="http://purl.obolibrary.org/obo/GAZ_00053704">
        <obo:RO_0001025 rdf:resource="http://purl.obolibrary.org/obo/GAZ_00053685"/>
        <obo:IAO_0000115>A volcanic cone.</obo:IAO_0000115>
        <oboInOwl:hasOBONamespace>GAZ</oboInOwl:hasOBONamespace>
        <oboInOwl:id>GAZ:00053704</oboInOwl:id>
        <rdfs:label>Tell el Antoor</rdfs:label>
    </owl:NamedIndividual>
    


    <!-- http://purl.obolibrary.org/obo/GAZ_00053705 -->

    <owl:NamedIndividual rdf:about="http://purl.obolibrary.org/obo/GAZ_00053705">
        <obo:RO_0001025 rdf:resource="http://purl.obolibrary.org/obo/GAZ_00053685"/>
        <obo:IAO_0000115>A volcanic cone.</obo:IAO_0000115>
        <oboInOwl:hasOBONamespace>GAZ</oboInOwl:hasOBONamespace>
        <oboInOwl:id>GAZ:00053705</oboInOwl:id>
        <rdfs:label>Tell Um Rqeibi</rdfs:label>
    </owl:NamedIndividual>
    


    <!-- http://purl.obolibrary.org/obo/GAZ_00053706 -->

    <owl:NamedIndividual rdf:about="http://purl.obolibrary.org/obo/GAZ_00053706">
        <obo:RO_0001025 rdf:resource="http://purl.obolibrary.org/obo/GAZ_00053685"/>
        <obo:IAO_0000115>A volcanic cone.</obo:IAO_0000115>
        <oboInOwl:hasOBONamespace>GAZ</oboInOwl:hasOBONamespace>
        <oboInOwl:id>GAZ:00053706</oboInOwl:id>
        <rdfs:label>Tell Qebli</rdfs:label>
    </owl:NamedIndividual>
    


    <!-- http://purl.obolibrary.org/obo/GAZ_00053707 -->

    <owl:NamedIndividual rdf:about="http://purl.obolibrary.org/obo/GAZ_00053707">
        <obo:RO_0001025 rdf:resource="http://purl.obolibrary.org/obo/GAZ_00053685"/>
        <obo:IAO_0000115>A volcanic cone.</obo:IAO_0000115>
        <oboInOwl:hasOBONamespace>GAZ</oboInOwl:hasOBONamespace>
        <oboInOwl:id>GAZ:00053707</oboInOwl:id>
        <rdfs:label>Tell As Skhana</rdfs:label>
    </owl:NamedIndividual>
    


    <!-- http://purl.obolibrary.org/obo/GAZ_00053708 -->

    <owl:NamedIndividual rdf:about="http://purl.obolibrary.org/obo/GAZ_00053708">
        <obo:IAO_0000115>A large basaltic volcanic field in northwestern Saudi Arabia near the Jordanian border, covers an area of 15,200 sq km. The volcanic field forms the southern third of the massive Harrat Ash Shamah volcanic field, which extends from Syria through Jordan into northern Saudi Arabia. The Saudi Arabian portion of the Harrat Ash Shamah volcanic field extends across a 210 km-long, roughly 75 km wide NW-SE-trending area on the NE flanks of the Wadi Sirhan and reaches its 1100 m high point at Jabal al Amud.</obo:IAO_0000115>
        <oboInOwl:hasOBONamespace>GAZ</oboInOwl:hasOBONamespace>
        <oboInOwl:id>GAZ:00053708</oboInOwl:id>
        <rdfs:label>Al Harrah Volcanic Field</rdfs:label>
    </owl:NamedIndividual>
    


    <!-- http://purl.obolibrary.org/obo/GAZ_00053709 -->

    <owl:NamedIndividual rdf:about="http://purl.obolibrary.org/obo/GAZ_00053709">
        <obo:RO_0001025 rdf:resource="http://purl.obolibrary.org/obo/GAZ_00015054"/>
        <obo:IAO_0000115>The northernmost of a series of Quaternary volcanic fields paralleling the Red Sea coast of Saudi Arabia. The olivine basaltic volcanic field of Harrat ar Raha lies south of the Plain of El-&apos;Hisma, south of the town of Tabuk.</obo:IAO_0000115>
        <oboInOwl:hasOBONamespace>GAZ</oboInOwl:hasOBONamespace>
        <oboInOwl:id>GAZ:00053709</oboInOwl:id>
        <rdfs:label>Harrat ar Rahah Volcanic Field</rdfs:label>
    </owl:NamedIndividual>
    


    <!-- http://purl.obolibrary.org/obo/GAZ_00053710 -->

    <owl:NamedIndividual rdf:about="http://purl.obolibrary.org/obo/GAZ_00053710">
        <obo:RO_0001025 rdf:resource="http://purl.obolibrary.org/obo/GAZ_00015060"/>
        <obo:IAO_0000115>A volcanic field located in NW Saudi Arabia. It contains young basaltic scoria and tuff cones and associated lava fields. The massive alkali olivine basaltic lava field reaches a height of 1920 m; it extends about 125 km in a NW-SE direction and is contiguous with the Harrat ar Rahat volcanic field to the NW.</obo:IAO_0000115>
        <oboInOwl:hasOBONamespace>GAZ</oboInOwl:hasOBONamespace>
        <oboInOwl:id>GAZ:00053710</oboInOwl:id>
        <rdfs:label>Harrat &apos;Uwayrid Volcanic Field</rdfs:label>
    </owl:NamedIndividual>
    


    <!-- http://purl.obolibrary.org/obo/GAZ_00053711 -->

    <owl:NamedIndividual rdf:about="http://purl.obolibrary.org/obo/GAZ_00053711">
        <obo:RO_0001025 rdf:resource="http://purl.obolibrary.org/obo/GAZ_00015054"/>
        <obo:IAO_0000115>A basaltic volcanic field in NW Saudi Arabia, east of the Red Sea port of Umm Lajj. It contains about 50 volcanic cones that were constructed over Precambrian crystalline rocks along a N-S axis. Harrat Lunayyir is one of the smallest of the Holocene lava fields of Saudi Arabia, but individual flow lobes radiate long distances from the center of the Harrat, and flows reached the Red Sea in two places. Lava flows are basaltic to basanitic in composition, and the Holocene flows are alkali olivine basalts.</obo:IAO_0000115>
        <oboInOwl:hasOBONamespace>GAZ</oboInOwl:hasOBONamespace>
        <oboInOwl:id>GAZ:00053711</oboInOwl:id>
        <rdfs:label>Harrat Lunayyir Volcanic Field</rdfs:label>
    </owl:NamedIndividual>
    


    <!-- http://purl.obolibrary.org/obo/GAZ_00053712 -->

    <owl:NamedIndividual rdf:about="http://purl.obolibrary.org/obo/GAZ_00053712">
        <obo:RO_0001025 rdf:resource="http://purl.obolibrary.org/obo/GAZ_00015061"/>
        <obo:IAO_0000115>A volcanic field that contains scattered shield volcanoes and scoria cones. It merges with the much larger Harrat Khaybar volcanic field to the south. The Harrat Ithnayn volcanic field overlies Cambrian sandstones and Precambrian basement rocks. Vents of Harrat Ithnayn form a general N-S pattern, but are more scattered than those of Harrat Khaybar. Harrat Ithnayn rocks are of basaltic and basanitic composition and lack the silicic components present in neighboring Harrat Khaybar.</obo:IAO_0000115>
        <oboInOwl:hasOBONamespace>GAZ</oboInOwl:hasOBONamespace>
        <oboInOwl:id>GAZ:00053712</oboInOwl:id>
        <rdfs:label>Harrat Ithnayn Volcanic Field</rdfs:label>
    </owl:NamedIndividual>
    


    <!-- http://purl.obolibrary.org/obo/GAZ_00053713 -->

    <owl:NamedIndividual rdf:about="http://purl.obolibrary.org/obo/GAZ_00053713">
        <obo:RO_0001025 rdf:resource="http://purl.obolibrary.org/obo/GAZ_00015060"/>
        <obo:IAO_0000115>A volcanic field that covers an area of more than 14,000 km2 north of Madinah (Medina). A spectacular 100 km-long N-S linear vent system contains felsic lava domes, tuff rings, the Jabal Qidr stratovolcano, as well as numerous small basaltic cones. At least seven post-neolithic (&lt;4500 years old) and eight &quot;historical&quot; (&lt;1500 years old) lava flows are present. In the latter category is the prominent 55 km-long Habir lava flow as well as Jabal Qidr stratovolcano, the only stratovolcano in the Harrats of western Saudi Arabia.</obo:IAO_0000115>
        <oboInOwl:hasOBONamespace>GAZ</oboInOwl:hasOBONamespace>
        <oboInOwl:id>GAZ:00053713</oboInOwl:id>
        <rdfs:label>Harrat Khaybar Volcanic Field</rdfs:label>
    </owl:NamedIndividual>
    


    <!-- http://purl.obolibrary.org/obo/GAZ_00053714 -->

    <owl:NamedIndividual rdf:about="http://purl.obolibrary.org/obo/GAZ_00053714">
        <obo:RO_0001025 rdf:resource="http://purl.obolibrary.org/obo/GAZ_00053713"/>
        <obo:IAO_0000115>A stratovolcano.</obo:IAO_0000115>
        <oboInOwl:hasOBONamespace>GAZ</oboInOwl:hasOBONamespace>
        <oboInOwl:id>GAZ:00053714</oboInOwl:id>
        <rdfs:label>Jabal Qidr Volcano</rdfs:label>
    </owl:NamedIndividual>
    


    <!-- http://purl.obolibrary.org/obo/GAZ_00053715 -->

    <owl:NamedIndividual rdf:about="http://purl.obolibrary.org/obo/GAZ_00053715">
        <obo:RO_0001025 rdf:resource="http://purl.obolibrary.org/obo/GAZ_00007506"/>
        <obo:IAO_0000115>A volcanic field that extends for 300 km south of the holy city of Al Madinah (Medina). Four coalescing lava fields erupted from offset NNW-trending vent systems comprise Harrat Rahat, which has an average width of 60 km. Lava flows extend as far as 100 km west of the axis of the field. Basaltic scoria cones dominate Harrat Rahat, but the volcanic field has also produced more silicic trachy-basaltic to trachytic rocks. Small shield volcanoes and pelean-type lava domes with associated pyroclastic-flow and -surge deposits are also present.</obo:IAO_0000115>
        <oboInOwl:hasOBONamespace>GAZ</oboInOwl:hasOBONamespace>
        <oboInOwl:id>GAZ:00053715</oboInOwl:id>
        <rdfs:label>Harrat Rahat Volcanic Field</rdfs:label>
    </owl:NamedIndividual>
    


    <!-- http://purl.obolibrary.org/obo/GAZ_00053716 -->

    <owl:NamedIndividual rdf:about="http://purl.obolibrary.org/obo/GAZ_00053716">
        <obo:RO_0001025 rdf:resource="http://purl.obolibrary.org/obo/GAZ_00015060"/>
        <obo:IAO_0000115>A volcanic field, located east of a N-S-trending line of volcanic fields in central Saudi Arabia. It is comprised of basaltic scoria cones, tuff rings and maars, and phonolitic lava domes and flows. Most of Harrat Kishb is of Pleistocene age; Holocene flows are restricted to three areas in the western half of the field. Jabal Aslaj cone and its associated lava flows contain abundant granitic blocks from basement rocks and ultramafic nodules. Jabal Hil is a large scoria cone with a 300-m-wide crater that was filled and overtopped by a lava lake. Harrat Kishb includes several tuff rings and maars, including the 800 x 600 m wide Al Wabah maar in the west-central part of the Harrat.</obo:IAO_0000115>
        <oboInOwl:hasOBONamespace>GAZ</oboInOwl:hasOBONamespace>
        <oboInOwl:id>GAZ:00053716</oboInOwl:id>
        <rdfs:label>Harrat Kishb Volcanic Field</rdfs:label>
    </owl:NamedIndividual>
    


    <!-- http://purl.obolibrary.org/obo/GAZ_00053717 -->

    <owl:NamedIndividual rdf:about="http://purl.obolibrary.org/obo/GAZ_00053717">
        <obo:RO_0001025 rdf:resource="http://purl.obolibrary.org/obo/GAZ_00007506"/>
        <obo:IAO_0000115>A volcanic field that lies directly along the Red Sea coast. It covers an 1800 km2 area west of the town of Abha and separates the Tihamat ash Sham and Tihamat &apos;Asir coastal plains.</obo:IAO_0000115>
        <oboInOwl:hasOBONamespace>GAZ</oboInOwl:hasOBONamespace>
        <oboInOwl:id>GAZ:00053717</oboInOwl:id>
        <rdfs:label>Harrat al Birk Volcanic Field</rdfs:label>
    </owl:NamedIndividual>
    


    <!-- http://purl.obolibrary.org/obo/GAZ_00053718 -->

    <owl:NamedIndividual rdf:about="http://purl.obolibrary.org/obo/GAZ_00053718">
        <obo:RO_0001025 rdf:resource="http://purl.obolibrary.org/obo/GAZ_00010398"/>
        <obo:IAO_0000115>A small olivine basaltic volcanic field along the Red Sea coast at the SW tip of Saudi Arabia. It contains three groups of volcanoes, Qummatain, Djar&apos;atain-Harra, and &apos;Ukwatain. Hot springs occur south of Djar&apos;atain and between it and &apos;Ukwatain.</obo:IAO_0000115>
        <oboInOwl:hasOBONamespace>GAZ</oboInOwl:hasOBONamespace>
        <oboInOwl:id>GAZ:00053718</oboInOwl:id>
        <rdfs:label>Jabal Yar Volcanic Field</rdfs:label>
    </owl:NamedIndividual>
    


    <!-- http://purl.obolibrary.org/obo/GAZ_00053719 -->

    <owl:NamedIndividual rdf:about="http://purl.obolibrary.org/obo/GAZ_00053719">
        <obo:RO_0001025 rdf:resource="http://purl.obolibrary.org/obo/GAZ_00053718"/>
        <oboInOwl:hasOBONamespace>GAZ</oboInOwl:hasOBONamespace>
        <oboInOwl:id>GAZ:00053719</oboInOwl:id>
        <rdfs:label>Qummatain Volcanoes</rdfs:label>
    </owl:NamedIndividual>
    


    <!-- http://purl.obolibrary.org/obo/GAZ_00053720 -->

    <owl:NamedIndividual rdf:about="http://purl.obolibrary.org/obo/GAZ_00053720">
        <obo:RO_0001025 rdf:resource="http://purl.obolibrary.org/obo/GAZ_00053718"/>
        <oboInOwl:hasOBONamespace>GAZ</oboInOwl:hasOBONamespace>
        <oboInOwl:id>GAZ:00053720</oboInOwl:id>
        <rdfs:label>Djar&apos;atain-Harra Volcanoes</rdfs:label>
    </owl:NamedIndividual>
    


    <!-- http://purl.obolibrary.org/obo/GAZ_00053721 -->

    <owl:NamedIndividual rdf:about="http://purl.obolibrary.org/obo/GAZ_00053721">
        <obo:RO_0001025 rdf:resource="http://purl.obolibrary.org/obo/GAZ_00053718"/>
        <oboInOwl:hasOBONamespace>GAZ</oboInOwl:hasOBONamespace>
        <oboInOwl:id>GAZ:00053721</oboInOwl:id>
        <rdfs:label>&apos;Ukwatain Volcanoes</rdfs:label>
    </owl:NamedIndividual>
    


    <!-- http://purl.obolibrary.org/obo/GAZ_00053728 -->

    <owl:NamedIndividual rdf:about="http://purl.obolibrary.org/obo/GAZ_00053728">
        <obo:RO_0001025 rdf:resource="http://purl.obolibrary.org/obo/GAZ_00005295"/>
        <obo:IAO_0000115>An island in the Persian Gulf.</obo:IAO_0000115>
        <oboInOwl:hasOBONamespace>GAZ</oboInOwl:hasOBONamespace>
        <oboInOwl:id>GAZ:00053728</oboInOwl:id>
        <rdfs:label>Shidvar Island</rdfs:label>
    </owl:NamedIndividual>
    


    <!-- http://purl.obolibrary.org/obo/GAZ_00057488 -->

    <owl:NamedIndividual rdf:about="http://purl.obolibrary.org/obo/GAZ_00057488">
        <obo:IAO_0000115>The S part of the Sarawat Mountains.</obo:IAO_0000115>
        <oboInOwl:hasOBONamespace>GAZ</oboInOwl:hasOBONamespace>
        <oboInOwl:id>GAZ:00057488</oboInOwl:id>
        <rdfs:label>Sarat &apos;Asir</rdfs:label>
    </owl:NamedIndividual>
    


    <!-- http://purl.obolibrary.org/obo/GAZ_00057489 -->

    <owl:NamedIndividual rdf:about="http://purl.obolibrary.org/obo/GAZ_00057489">
        <obo:IAO_0000115>The N part of the Sarawat Mountains.</obo:IAO_0000115>
        <oboInOwl:hasOBONamespace>GAZ</oboInOwl:hasOBONamespace>
        <oboInOwl:id>GAZ:00057489</oboInOwl:id>
        <rdfs:label>Sarat al-Hejaz</rdfs:label>
    </owl:NamedIndividual>
    


    <!-- http://purl.obolibrary.org/obo/GAZ_00057490 -->

    <owl:NamedIndividual rdf:about="http://purl.obolibrary.org/obo/GAZ_00057490">
        <obo:IAO_0000115>The S part of the Sarawat Mountains.</obo:IAO_0000115>
        <oboInOwl:hasOBONamespace>GAZ</oboInOwl:hasOBONamespace>
        <oboInOwl:id>GAZ:00057490</oboInOwl:id>
        <rdfs:label>Sarat al-Yemen</rdfs:label>
    </owl:NamedIndividual>
    


    <!-- http://purl.obolibrary.org/obo/GAZ_00058383 -->

    <owl:NamedIndividual rdf:about="http://purl.obolibrary.org/obo/GAZ_00058383">
        <obo:RO_0001025 rdf:resource="http://purl.obolibrary.org/obo/GAZ_00053683"/>
        <obo:IAO_0000115>A crater lake in the northeastern Golan Heights, near Mount Hermon.</obo:IAO_0000115>
        <oboInOwl:hasOBONamespace>GAZ</oboInOwl:hasOBONamespace>
        <oboInOwl:id>GAZ:00058383</oboInOwl:id>
        <rdfs:label>Birkat Ram</rdfs:label>
    </owl:NamedIndividual>
    


    <!-- http://purl.obolibrary.org/obo/GAZ_00078574 -->

    <owl:NamedIndividual rdf:about="http://purl.obolibrary.org/obo/GAZ_00078574">
        <obo:RO_0001025 rdf:resource="http://purl.obolibrary.org/obo/GAZ_00005295"/>
        <obo:IAO_0000115>A natural island 600 m off the coast of Abu Dhabi island.</obo:IAO_0000115>
        <oboInOwl:hasOBONamespace>GAZ</oboInOwl:hasOBONamespace>
        <oboInOwl:id>GAZ:00078574</oboInOwl:id>
        <rdfs:label>Al Reem Island</rdfs:label>
    </owl:NamedIndividual>
    


    <!-- http://purl.obolibrary.org/obo/GAZ_00078575 -->

    <owl:NamedIndividual rdf:about="http://purl.obolibrary.org/obo/GAZ_00078575">
        <obo:RO_0001025 rdf:resource="http://purl.obolibrary.org/obo/GAZ_00005295"/>
        <obo:IAO_0000115>A large, low lying island 500 m off the coast of Abu Dhabi island.</obo:IAO_0000115>
        <oboInOwl:hasOBONamespace>GAZ</oboInOwl:hasOBONamespace>
        <oboInOwl:id>GAZ:00078575</oboInOwl:id>
        <rdfs:label>Saadiyat Island</rdfs:label>
    </owl:NamedIndividual>
    


    <!-- http://purl.obolibrary.org/obo/GAZ_00078576 -->

    <owl:NamedIndividual rdf:about="http://purl.obolibrary.org/obo/GAZ_00078576">
        <obo:RO_0001025 rdf:resource="http://purl.obolibrary.org/obo/GAZ_00005295"/>
        <oboInOwl:hasOBONamespace>GAZ</oboInOwl:hasOBONamespace>
        <oboInOwl:id>GAZ:00078576</oboInOwl:id>
        <rdfs:label>Abu Dhabi Island</rdfs:label>
    </owl:NamedIndividual>
    


    <!-- http://purl.obolibrary.org/obo/GAZ_00078583 -->

    <owl:NamedIndividual rdf:about="http://purl.obolibrary.org/obo/GAZ_00078583">
        <obo:RO_0001025 rdf:resource="http://purl.obolibrary.org/obo/GAZ_00005295"/>
        <obo:IAO_0000115>A mangrove island S of Kalba.</obo:IAO_0000115>
        <oboInOwl:hasOBONamespace>GAZ</oboInOwl:hasOBONamespace>
        <oboInOwl:id>GAZ:00078583</oboInOwl:id>
        <rdfs:label>Khor Kalba</rdfs:label>
    </owl:NamedIndividual>
    


    <!-- http://purl.obolibrary.org/obo/GAZ_00078658 -->

    <owl:NamedIndividual rdf:about="http://purl.obolibrary.org/obo/GAZ_00078658">
        <rdf:type rdf:resource="http://purl.obolibrary.org/obo/ENVO_00000856"/>
        <obo:RO_0001025 rdf:resource="http://purl.obolibrary.org/obo/GAZ_02000358"/>
        <obo:RO_0001025 rdf:resource="http://purl.obolibrary.org/obo/GAZ_02000360"/>
        <obo:IAO_0000115>A municipality in the Northern and Southern Governorates.</obo:IAO_0000115>
        <oboInOwl:hasOBONamespace>GAZ</oboInOwl:hasOBONamespace>
        <oboInOwl:id>GAZ:00078658</oboInOwl:id>
        <rdfs:label>Municipality of Al Mintaqah al Gharbiyah</rdfs:label>
    </owl:NamedIndividual>
    


    <!-- http://purl.obolibrary.org/obo/GAZ_00078659 -->

    <owl:NamedIndividual rdf:about="http://purl.obolibrary.org/obo/GAZ_00078659">
        <rdf:type rdf:resource="http://purl.obolibrary.org/obo/ENVO_00000856"/>
        <obo:RO_0001025 rdf:resource="http://purl.obolibrary.org/obo/GAZ_02000358"/>
        <obo:RO_0001025 rdf:resource="http://purl.obolibrary.org/obo/GAZ_02000361"/>
        <obo:IAO_0000115>A municipality in the Central and Southern Governorates.</obo:IAO_0000115>
        <oboInOwl:hasOBONamespace>GAZ</oboInOwl:hasOBONamespace>
        <oboInOwl:id>GAZ:00078659</oboInOwl:id>
        <rdfs:label>Municipality of Ar Rifa&apos; wa al Mintaqah al Janubiyah</rdfs:label>
    </owl:NamedIndividual>
    


    <!-- http://purl.obolibrary.org/obo/GAZ_00078660 -->

    <owl:NamedIndividual rdf:about="http://purl.obolibrary.org/obo/GAZ_00078660">
        <obo:RO_0001025 rdf:resource="http://purl.obolibrary.org/obo/GAZ_02000358"/>
        <oboInOwl:hasOBONamespace>GAZ</oboInOwl:hasOBONamespace>
        <oboInOwl:id>GAZ:00078660</oboInOwl:id>
        <rdfs:label>Municipality of Juzur Hawar</rdfs:label>
    </owl:NamedIndividual>
    


    <!-- http://purl.obolibrary.org/obo/GAZ_00078661 -->

    <owl:NamedIndividual rdf:about="http://purl.obolibrary.org/obo/GAZ_00078661">
        <obo:RO_0001025 rdf:resource="http://purl.obolibrary.org/obo/GAZ_00005295"/>
        <obo:RO_0001025 rdf:resource="http://purl.obolibrary.org/obo/GAZ_00006936"/>
        <obo:RO_0001025 rdf:resource="http://purl.obolibrary.org/obo/GAZ_00078660"/>
        <obo:IAO_0000115>A group of islands situated off the west coast of Qatar in the Gulf of Bahrain of the Persian Gulf. Despite their proximity to Qatar (Suwad al Janubiyah is only 1.4 km from the Qatari mainland at the peninsula of Ras Abruq, while Rubud Al Gharbiyah, the island closest to the main island of Bahrain, lies at a distance of 19.7 km to it), the islands belong to Bahrain. A Ramsar Site.</obo:IAO_0000115>
        <oboInOwl:hasOBONamespace>GAZ</oboInOwl:hasOBONamespace>
        <oboInOwl:id>GAZ:00078661</oboInOwl:id>
        <rdfs:label>Hawar Islands</rdfs:label>
    </owl:NamedIndividual>
    


    <!-- http://purl.obolibrary.org/obo/GAZ_00078662 -->

    <owl:NamedIndividual rdf:about="http://purl.obolibrary.org/obo/GAZ_00078662">
        <obo:RO_0001025 rdf:resource="http://purl.obolibrary.org/obo/GAZ_00078661"/>
        <obo:IAO_0000115>An island in the Hawar Islands.</obo:IAO_0000115>
        <oboInOwl:hasOBONamespace>GAZ</oboInOwl:hasOBONamespace>
        <oboInOwl:id>GAZ:00078662</oboInOwl:id>
        <rdfs:label>Rubud Al Gharbiyah</rdfs:label>
    </owl:NamedIndividual>
    


    <!-- http://purl.obolibrary.org/obo/GAZ_00078663 -->

    <owl:NamedIndividual rdf:about="http://purl.obolibrary.org/obo/GAZ_00078663">
        <obo:RO_0001025 rdf:resource="http://purl.obolibrary.org/obo/GAZ_00078661"/>
        <obo:IAO_0000115>An island in the Hawar Islands.</obo:IAO_0000115>
        <oboInOwl:hasOBONamespace>GAZ</oboInOwl:hasOBONamespace>
        <oboInOwl:id>GAZ:00078663</oboInOwl:id>
        <rdfs:label>Rubud Al Sharqiyah</rdfs:label>
    </owl:NamedIndividual>
    


    <!-- http://purl.obolibrary.org/obo/GAZ_00078664 -->

    <owl:NamedIndividual rdf:about="http://purl.obolibrary.org/obo/GAZ_00078664">
        <obo:RO_0001025 rdf:resource="http://purl.obolibrary.org/obo/GAZ_00078661"/>
        <obo:IAO_0000115>An island in the Hawar Islands.</obo:IAO_0000115>
        <oboInOwl:hasOBONamespace>GAZ</oboInOwl:hasOBONamespace>
        <oboInOwl:id>GAZ:00078664</oboInOwl:id>
        <rdfs:label>Umm Jinni</rdfs:label>
    </owl:NamedIndividual>
    


    <!-- http://purl.obolibrary.org/obo/GAZ_00078665 -->

    <owl:NamedIndividual rdf:about="http://purl.obolibrary.org/obo/GAZ_00078665">
        <obo:RO_0001025 rdf:resource="http://purl.obolibrary.org/obo/GAZ_00078661"/>
        <obo:IAO_0000115>A group of islands in the Hawar Islands.</obo:IAO_0000115>
        <oboInOwl:hasOBONamespace>GAZ</oboInOwl:hasOBONamespace>
        <oboInOwl:id>GAZ:00078665</oboInOwl:id>
        <rdfs:label>Al Hajiyat</rdfs:label>
    </owl:NamedIndividual>
    


    <!-- http://purl.obolibrary.org/obo/GAZ_00078666 -->

    <owl:NamedIndividual rdf:about="http://purl.obolibrary.org/obo/GAZ_00078666">
        <obo:RO_0001025 rdf:resource="http://purl.obolibrary.org/obo/GAZ_00078661"/>
        <obo:IAO_0000115>An island in the Hawar Islands.</obo:IAO_0000115>
        <oboInOwl:hasOBONamespace>GAZ</oboInOwl:hasOBONamespace>
        <oboInOwl:id>GAZ:00078666</oboInOwl:id>
        <rdfs:label>Ajirah</rdfs:label>
    </owl:NamedIndividual>
    


    <!-- http://purl.obolibrary.org/obo/GAZ_00078667 -->

    <owl:NamedIndividual rdf:about="http://purl.obolibrary.org/obo/GAZ_00078667">
        <obo:RO_0001025 rdf:resource="http://purl.obolibrary.org/obo/GAZ_00078661"/>
        <obo:IAO_0000115>An island in the Hawar Islands.</obo:IAO_0000115>
        <oboInOwl:hasOBONamespace>GAZ</oboInOwl:hasOBONamespace>
        <oboInOwl:id>GAZ:00078667</oboInOwl:id>
        <rdfs:label>Suwad al Janubiyah</rdfs:label>
    </owl:NamedIndividual>
    


    <!-- http://purl.obolibrary.org/obo/GAZ_00078668 -->

    <owl:NamedIndividual rdf:about="http://purl.obolibrary.org/obo/GAZ_00078668">
        <obo:RO_0001025 rdf:resource="http://purl.obolibrary.org/obo/GAZ_00078661"/>
        <obo:IAO_0000115>An island in the Hawar Islands.</obo:IAO_0000115>
        <oboInOwl:hasOBONamespace>GAZ</oboInOwl:hasOBONamespace>
        <oboInOwl:id>GAZ:00078668</oboInOwl:id>
        <rdfs:label>Umm Kharurah</rdfs:label>
    </owl:NamedIndividual>
    


    <!-- http://purl.obolibrary.org/obo/GAZ_00078669 -->

    <owl:NamedIndividual rdf:about="http://purl.obolibrary.org/obo/GAZ_00078669">
        <obo:RO_0001025 rdf:resource="http://purl.obolibrary.org/obo/GAZ_00078661"/>
        <obo:IAO_0000115>Isolated sea stacks with shingle beaches with surrounding shallow lagoon in the Hawar Islands.</obo:IAO_0000115>
        <oboInOwl:hasOBONamespace>GAZ</oboInOwl:hasOBONamespace>
        <oboInOwl:id>GAZ:00078669</oboInOwl:id>
        <rdfs:label>al Wukur</rdfs:label>
    </owl:NamedIndividual>
    


    <!-- http://purl.obolibrary.org/obo/GAZ_00078670 -->

    <owl:NamedIndividual rdf:about="http://purl.obolibrary.org/obo/GAZ_00078670">
        <obo:RO_0001025 rdf:resource="http://purl.obolibrary.org/obo/GAZ_00078661"/>
        <obo:IAO_0000115>A group of islands in the Hawar Islands.</obo:IAO_0000115>
        <oboInOwl:hasOBONamespace>GAZ</oboInOwl:hasOBONamespace>
        <oboInOwl:id>GAZ:00078670</oboInOwl:id>
        <rdfs:label>Bu Tammur</rdfs:label>
    </owl:NamedIndividual>
    


    <!-- http://purl.obolibrary.org/obo/GAZ_00078671 -->

    <owl:NamedIndividual rdf:about="http://purl.obolibrary.org/obo/GAZ_00078671">
        <obo:RO_0001025 rdf:resource="http://purl.obolibrary.org/obo/GAZ_00078661"/>
        <obo:IAO_0000115>An island in the Hawar Islands.</obo:IAO_0000115>
        <oboInOwl:hasOBONamespace>GAZ</oboInOwl:hasOBONamespace>
        <oboInOwl:id>GAZ:00078671</oboInOwl:id>
        <rdfs:label>Muhazwarah</rdfs:label>
    </owl:NamedIndividual>
    


    <!-- http://purl.obolibrary.org/obo/GAZ_00078672 -->

    <owl:NamedIndividual rdf:about="http://purl.obolibrary.org/obo/GAZ_00078672">
        <obo:RO_0001025 rdf:resource="http://purl.obolibrary.org/obo/GAZ_00078661"/>
        <obo:IAO_0000115>An island in the Hawar Islands.</obo:IAO_0000115>
        <oboInOwl:hasOBONamespace>GAZ</oboInOwl:hasOBONamespace>
        <oboInOwl:id>GAZ:00078672</oboInOwl:id>
        <rdfs:label>Suwad ash Shamaliyah</rdfs:label>
    </owl:NamedIndividual>
    


    <!-- http://purl.obolibrary.org/obo/GAZ_00078673 -->

    <owl:NamedIndividual rdf:about="http://purl.obolibrary.org/obo/GAZ_00078673">
        <obo:RO_0001025 rdf:resource="http://purl.obolibrary.org/obo/GAZ_00078661"/>
        <obo:IAO_0000115>A group of islands in the Hawar Islands.</obo:IAO_0000115>
        <oboInOwl:hasOBONamespace>GAZ</oboInOwl:hasOBONamespace>
        <oboInOwl:id>GAZ:00078673</oboInOwl:id>
        <rdfs:label>Bu Sadad</rdfs:label>
    </owl:NamedIndividual>
    


    <!-- http://purl.obolibrary.org/obo/GAZ_00078674 -->

    <owl:NamedIndividual rdf:about="http://purl.obolibrary.org/obo/GAZ_00078674">
        <obo:RO_0001025 rdf:resource="http://purl.obolibrary.org/obo/GAZ_00078661"/>
        <obo:IAO_0000115>An island in the Hawar Islands.</obo:IAO_0000115>
        <oboInOwl:hasOBONamespace>GAZ</oboInOwl:hasOBONamespace>
        <oboInOwl:id>GAZ:00078674</oboInOwl:id>
        <rdfs:label>Jazirat Jinan</rdfs:label>
    </owl:NamedIndividual>
    


    <!-- http://purl.obolibrary.org/obo/GAZ_00078675 -->

    <owl:NamedIndividual rdf:about="http://purl.obolibrary.org/obo/GAZ_00078675">
        <rdf:type rdf:resource="http://purl.obolibrary.org/obo/ENVO_00000856"/>
        <obo:RO_0001025 rdf:resource="http://purl.obolibrary.org/obo/GAZ_02000360"/>
        <obo:RO_0001025 rdf:resource="http://purl.obolibrary.org/obo/GAZ_02000361"/>
        <obo:IAO_0000115>A municipality of Bahrain in the northern part of the country. Its territory is now in the Central and Northern Governorates.</obo:IAO_0000115>
        <oboInOwl:hasOBONamespace>GAZ</oboInOwl:hasOBONamespace>
        <oboInOwl:id>GAZ:00078675</oboInOwl:id>
        <rdfs:label>Municipality of Al Mintaqah al Wusta</rdfs:label>
    </owl:NamedIndividual>
    


    <!-- http://purl.obolibrary.org/obo/GAZ_00078676 -->

    <owl:NamedIndividual rdf:about="http://purl.obolibrary.org/obo/GAZ_00078676">
        <rdf:type rdf:resource="http://purl.obolibrary.org/obo/ENVO_00000856"/>
        <obo:RO_0001025 rdf:resource="http://purl.obolibrary.org/obo/GAZ_02000360"/>
        <obo:RO_0001025 rdf:resource="http://purl.obolibrary.org/obo/GAZ_02000362"/>
        <obo:IAO_0000115>A municipality in northern Bahrain. It was split off of the municipality of Ar Rifa&apos; wa al Mintaqah al Janubiyah in 1991.</obo:IAO_0000115>
        <oboInOwl:hasOBONamespace>GAZ</oboInOwl:hasOBONamespace>
        <oboInOwl:id>GAZ:00078676</oboInOwl:id>
        <rdfs:label>Municipality of Madinat Hamad</rdfs:label>
    </owl:NamedIndividual>
    


    <!-- http://purl.obolibrary.org/obo/GAZ_00078677 -->

    <owl:NamedIndividual rdf:about="http://purl.obolibrary.org/obo/GAZ_00078677">
        <rdf:type rdf:resource="http://purl.obolibrary.org/obo/ENVO_00000856"/>
        <obo:RO_0001025 rdf:resource="http://purl.obolibrary.org/obo/GAZ_02000360"/>
        <obo:RO_0001025 rdf:resource="http://purl.obolibrary.org/obo/GAZ_02000362"/>
        <obo:IAO_0000115>A municipality in northern Bahrain. Now in the Capital and Northern Governorate.</obo:IAO_0000115>
        <oboInOwl:hasOBONamespace>GAZ</oboInOwl:hasOBONamespace>
        <oboInOwl:id>GAZ:00078677</oboInOwl:id>
        <rdfs:label>Municipality of Jidd Haffs</rdfs:label>
    </owl:NamedIndividual>
    


    <!-- http://purl.obolibrary.org/obo/GAZ_00078678 -->

    <owl:NamedIndividual rdf:about="http://purl.obolibrary.org/obo/GAZ_00078678">
        <rdf:type rdf:resource="http://purl.obolibrary.org/obo/ENVO_00000856"/>
        <obo:RO_0001025 rdf:resource="http://purl.obolibrary.org/obo/GAZ_02000360"/>
        <obo:IAO_0000115>A municipality of Bahrain in the northern part of the country. Its territory is now in the Northern Governorate.</obo:IAO_0000115>
        <oboInOwl:hasOBONamespace>GAZ</oboInOwl:hasOBONamespace>
        <oboInOwl:id>GAZ:00078678</oboInOwl:id>
        <rdfs:label>Municipality of Al Mintaqah al Shamaliyah</rdfs:label>
    </owl:NamedIndividual>
    


    <!-- http://purl.obolibrary.org/obo/GAZ_00078679 -->

    <owl:NamedIndividual rdf:about="http://purl.obolibrary.org/obo/GAZ_00078679">
        <obo:RO_0001025 rdf:resource="http://purl.obolibrary.org/obo/GAZ_00078676"/>
        <obo:IAO_0000115>The capital city of Bahrain.</obo:IAO_0000115>
        <oboInOwl:hasOBONamespace>GAZ</oboInOwl:hasOBONamespace>
        <oboInOwl:id>GAZ:00078679</oboInOwl:id>
        <rdfs:label>Manama</rdfs:label>
    </owl:NamedIndividual>
    


    <!-- http://purl.obolibrary.org/obo/GAZ_00078680 -->

    <owl:NamedIndividual rdf:about="http://purl.obolibrary.org/obo/GAZ_00078680">
        <rdf:type rdf:resource="http://purl.obolibrary.org/obo/ENVO_00000856"/>
        <obo:RO_0001025 rdf:resource="http://purl.obolibrary.org/obo/GAZ_02000359"/>
        <obo:IAO_0000115>A municipality in the Al Muharraq Governorate.</obo:IAO_0000115>
        <oboInOwl:hasOBONamespace>GAZ</oboInOwl:hasOBONamespace>
        <oboInOwl:id>GAZ:00078680</oboInOwl:id>
        <rdfs:label>Municipality of Al Muharraq</rdfs:label>
    </owl:NamedIndividual>
    


    <!-- http://purl.obolibrary.org/obo/GAZ_00078681 -->

    <owl:NamedIndividual rdf:about="http://purl.obolibrary.org/obo/GAZ_00078681">
        <rdf:type rdf:resource="http://purl.obolibrary.org/obo/ENVO_00000856"/>
        <obo:RO_0001025 rdf:resource="http://purl.obolibrary.org/obo/GAZ_02000359"/>
        <obo:IAO_0000115>A small municipality of Bahrain in the northeastern part of the country. Its territory is now in the Muharraq Governorate.</obo:IAO_0000115>
        <oboInOwl:hasOBONamespace>GAZ</oboInOwl:hasOBONamespace>
        <oboInOwl:id>GAZ:00078681</oboInOwl:id>
        <rdfs:label>Municipality of Al Hadd</rdfs:label>
    </owl:NamedIndividual>
    


    <!-- http://purl.obolibrary.org/obo/GAZ_00078682 -->

    <owl:NamedIndividual rdf:about="http://purl.obolibrary.org/obo/GAZ_00078682">
        <obo:RO_0001025 rdf:resource="http://purl.obolibrary.org/obo/GAZ_00078680"/>
        <obo:IAO_0000115>A man-made island near Al Muharraq.</obo:IAO_0000115>
        <oboInOwl:hasOBONamespace>GAZ</oboInOwl:hasOBONamespace>
        <oboInOwl:id>GAZ:00078682</oboInOwl:id>
        <rdfs:label>AMWAJ Island</rdfs:label>
    </owl:NamedIndividual>
    


    <!-- http://purl.obolibrary.org/obo/GAZ_00078683 -->

    <owl:NamedIndividual rdf:about="http://purl.obolibrary.org/obo/GAZ_00078683">
        <rdf:type rdf:resource="http://purl.obolibrary.org/obo/ENVO_00000856"/>
        <obo:RO_0001025 rdf:resource="http://purl.obolibrary.org/obo/GAZ_00006940"/>
        <obo:RO_0001025 rdf:resource="http://purl.obolibrary.org/obo/GAZ_02000361"/>
        <obo:IAO_0000115>A municipality in northeastern Bahrain. The region of Sitrah consists of the island of Sitrah and three villages close to it on the main island of Bahrain.</obo:IAO_0000115>
        <oboInOwl:hasOBONamespace>GAZ</oboInOwl:hasOBONamespace>
        <oboInOwl:id>GAZ:00078683</oboInOwl:id>
        <rdfs:label>Municipality of Sitrah</rdfs:label>
    </owl:NamedIndividual>
    


    <!-- http://purl.obolibrary.org/obo/GAZ_00078684 -->

    <owl:NamedIndividual rdf:about="http://purl.obolibrary.org/obo/GAZ_00078684">
        <rdf:type rdf:resource="http://purl.obolibrary.org/obo/ENVO_00000856"/>
        <obo:RO_0001025 rdf:resource="http://purl.obolibrary.org/obo/GAZ_02000361"/>
        <obo:IAO_0000115>A municipality located in the middle of Bahrain island, south of Isa town and north of Riffa.</obo:IAO_0000115>
        <oboInOwl:hasOBONamespace>GAZ</oboInOwl:hasOBONamespace>
        <oboInOwl:id>GAZ:00078684</oboInOwl:id>
        <rdfs:label>Municipality of A&apos;ali</rdfs:label>
    </owl:NamedIndividual>
    


    <!-- http://purl.obolibrary.org/obo/GAZ_00078685 -->

    <owl:NamedIndividual rdf:about="http://purl.obolibrary.org/obo/GAZ_00078685">
        <rdf:type rdf:resource="http://purl.obolibrary.org/obo/ENVO_00000856"/>
        <obo:RO_0001025 rdf:resource="http://purl.obolibrary.org/obo/GAZ_02000361"/>
        <obo:IAO_0000115>A municipality in Bahrain in the north central part of the country.</obo:IAO_0000115>
        <oboInOwl:hasOBONamespace>GAZ</oboInOwl:hasOBONamespace>
        <oboInOwl:id>GAZ:00078685</oboInOwl:id>
        <rdfs:label>Municipality of Madinat &apos;Isa</rdfs:label>
    </owl:NamedIndividual>
    


    <!-- http://purl.obolibrary.org/obo/GAZ_00089893 -->

    <owl:NamedIndividual rdf:about="http://purl.obolibrary.org/obo/GAZ_00089893">
        <obo:RO_0001025 rdf:resource="http://purl.obolibrary.org/obo/GAZ_00018504"/>
        <obo:IAO_0000115>A protected area including mangrove forests on the southern coast of Iran, particularly on and near the island of Qeshm in the Persian Gulf.</obo:IAO_0000115>
        <oboInOwl:hasOBONamespace>GAZ</oboInOwl:hasOBONamespace>
        <oboInOwl:id>GAZ:00089893</oboInOwl:id>
        <rdfs:label>Hara Protected Area</rdfs:label>
    </owl:NamedIndividual>
    


    <!-- http://purl.obolibrary.org/obo/GAZ_00102117 -->

    <owl:NamedIndividual rdf:about="http://purl.obolibrary.org/obo/GAZ_00102117">
        <obo:RO_0001025 rdf:resource="http://purl.obolibrary.org/obo/GAZ_00051269"/>
        <obo:IAO_0000115>The eastern side (3 km wide and 30 m deep) of the Bab-el-Mandeb straits separating Ras Menheli, Yemen, on the Arabian Peninsula and Ras Siyan, Djibouti, on the Horn of Africa. The Yemeni island of Perim divides the strait into two channels.</obo:IAO_0000115>
        <oboInOwl:hasOBONamespace>GAZ</oboInOwl:hasOBONamespace>
        <oboInOwl:id>GAZ:00102117</oboInOwl:id>
        <rdfs:label>Bab Iskender</rdfs:label>
    </owl:NamedIndividual>
    


    <!-- http://purl.obolibrary.org/obo/GAZ_00102118 -->

    <owl:NamedIndividual rdf:about="http://purl.obolibrary.org/obo/GAZ_00102118">
        <obo:RO_0001025 rdf:resource="http://purl.obolibrary.org/obo/GAZ_00051269"/>
        <obo:IAO_0000115>The western side of the Bab-el-Mandeb strait.</obo:IAO_0000115>
        <oboInOwl:hasOBONamespace>GAZ</oboInOwl:hasOBONamespace>
        <oboInOwl:id>GAZ:00102118</oboInOwl:id>
        <rdfs:label>Dact-el-Mayun</rdfs:label>
    </owl:NamedIndividual>
    


    <!-- http://purl.obolibrary.org/obo/GAZ_00124888 -->

    <owl:NamedIndividual rdf:about="http://purl.obolibrary.org/obo/GAZ_00124888">
        <obo:RO_0001025 rdf:resource="http://purl.obolibrary.org/obo/GAZ_00005295"/>
        <obo:IAO_0000115>A bay in the east of Bahrain, between Bahrain Island and Sitra island. The body of water is directly south of the Manama peninsula. The island of Nabih Saleh lies in the bay. A Ramsar Site.</obo:IAO_0000115>
        <oboInOwl:hasOBONamespace>GAZ</oboInOwl:hasOBONamespace>
        <oboInOwl:id>GAZ:00124888</oboInOwl:id>
        <rdfs:label>Tubli Bay</rdfs:label>
    </owl:NamedIndividual>
    


    <!-- http://purl.obolibrary.org/obo/GAZ_00144637 -->

    <owl:NamedIndividual rdf:about="http://purl.obolibrary.org/obo/GAZ_00144637">
        <obo:RO_0001025 rdf:resource="http://purl.obolibrary.org/obo/GAZ_00002456"/>
        <obo:IAO_0000115>An inlet of water on the Egyptian side of the Red Sea. It is located slightly north of the Tropic of Cancer. The northern part of Foul Bay is the Ras Banas peninsula.</obo:IAO_0000115>
        <oboInOwl:hasOBONamespace>GAZ</oboInOwl:hasOBONamespace>
        <oboInOwl:id>GAZ:00144637</oboInOwl:id>
        <rdfs:label>Foul Bay</rdfs:label>
    </owl:NamedIndividual>
    


    <!-- http://purl.obolibrary.org/obo/GAZ_00144638 -->

    <owl:NamedIndividual rdf:about="http://purl.obolibrary.org/obo/GAZ_00144638">
        <obo:RO_0001025 rdf:resource="http://purl.obolibrary.org/obo/GAZ_00144637"/>
        <obo:IAO_0000115>An island in Foul Bay.</obo:IAO_0000115>
        <oboInOwl:hasOBONamespace>GAZ</oboInOwl:hasOBONamespace>
        <oboInOwl:id>GAZ:00144638</oboInOwl:id>
        <rdfs:label>Rocky Island</rdfs:label>
    </owl:NamedIndividual>
    


    <!-- http://purl.obolibrary.org/obo/GAZ_00144639 -->

    <owl:NamedIndividual rdf:about="http://purl.obolibrary.org/obo/GAZ_00144639">
        <obo:RO_0001025 rdf:resource="http://purl.obolibrary.org/obo/GAZ_00144637"/>
        <obo:IAO_0000115>The largest of a group of islands in Foul Bay, Red Sea in Southern Egypt.</obo:IAO_0000115>
        <oboInOwl:hasOBONamespace>GAZ</oboInOwl:hasOBONamespace>
        <oboInOwl:id>GAZ:00144639</oboInOwl:id>
        <rdfs:label>Saint John&apos;s Island</rdfs:label>
    </owl:NamedIndividual>
    


    <!-- http://purl.obolibrary.org/obo/GAZ_00145310 -->

    <owl:NamedIndividual rdf:about="http://purl.obolibrary.org/obo/GAZ_00145310">
        <obo:RO_0001025 rdf:resource="http://purl.obolibrary.org/obo/GAZ_00005295"/>
        <obo:IAO_0000115>An inlet of the Persian Gulf on the east coast of Saudi Arabia, separated from the main body of water by the peninsula of Qatar. It surrounds the islands of Bahrain.</obo:IAO_0000115>
        <oboInOwl:hasOBONamespace>GAZ</oboInOwl:hasOBONamespace>
        <oboInOwl:id>GAZ:00145310</oboInOwl:id>
        <rdfs:label>Gulf of Bahrain</rdfs:label>
    </owl:NamedIndividual>
    


    <!-- http://purl.obolibrary.org/obo/GAZ_00145311 -->

    <owl:NamedIndividual rdf:about="http://purl.obolibrary.org/obo/GAZ_00145311">
        <obo:RO_0001025 rdf:resource="http://purl.obolibrary.org/obo/GAZ_00002456"/>
        <obo:IAO_0000115>A body of water on the Eritrean coastline on the Red Sea. The Gulf lies near the midpoint of the Eritrean coast, between the Foro province and the Buri Peninsula of the Ghelae&apos;lo province, both in the country&apos;s Northern Red Sea region.</obo:IAO_0000115>
        <oboInOwl:hasOBONamespace>GAZ</oboInOwl:hasOBONamespace>
        <oboInOwl:id>GAZ:00145311</oboInOwl:id>
        <rdfs:label>Gulf of Zula</rdfs:label>
    </owl:NamedIndividual>
    


    <!-- http://purl.obolibrary.org/obo/GAZ_00145498 -->

    <owl:NamedIndividual rdf:about="http://purl.obolibrary.org/obo/GAZ_00145498">
        <obo:RO_0001025 rdf:resource="http://purl.obolibrary.org/obo/GAZ_00005295"/>
        <obo:IAO_0000115>A saltwater creek located in Dubai, United Arab Emirates.</obo:IAO_0000115>
        <oboInOwl:hasOBONamespace>GAZ</oboInOwl:hasOBONamespace>
        <oboInOwl:id>GAZ:00145498</oboInOwl:id>
        <rdfs:label>Dubai Creek</rdfs:label>
    </owl:NamedIndividual>
    


    <!-- http://purl.obolibrary.org/obo/GAZ_00146201 -->

    <owl:NamedIndividual rdf:about="http://purl.obolibrary.org/obo/GAZ_00146201">
        <obo:RO_0001025 rdf:resource="http://purl.obolibrary.org/obo/GAZ_00002456"/>
        <obo:IAO_0000115>A bay on the Red Sea, off the coast of Eritrea.</obo:IAO_0000115>
        <oboInOwl:hasOBONamespace>GAZ</oboInOwl:hasOBONamespace>
        <oboInOwl:id>GAZ:00146201</oboInOwl:id>
        <rdfs:label>Amphila Bay</rdfs:label>
    </owl:NamedIndividual>
    


    <!-- http://purl.obolibrary.org/obo/GAZ_00146397 -->

    <owl:NamedIndividual rdf:about="http://purl.obolibrary.org/obo/GAZ_00146397">
        <obo:RO_0001025 rdf:resource="http://purl.obolibrary.org/obo/GAZ_00005295"/>
        <obo:IAO_0000115>A bay in Umm al Quwain.</obo:IAO_0000115>
        <oboInOwl:hasOBONamespace>GAZ</oboInOwl:hasOBONamespace>
        <oboInOwl:id>GAZ:00146397</oboInOwl:id>
        <rdfs:label>Khawr al Baydah</rdfs:label>
    </owl:NamedIndividual>
    


    <!-- http://purl.obolibrary.org/obo/GAZ_00176003 -->

    <owl:NamedIndividual rdf:about="http://purl.obolibrary.org/obo/GAZ_00176003">
        <obo:RO_0001025 rdf:resource="http://purl.obolibrary.org/obo/GAZ_00002456"/>
        <obo:IAO_0000115>A small 145 m long and 50 m wide artificial island in the Red Sea at the southern mouth of the Suez Canal.</obo:IAO_0000115>
        <oboInOwl:hasOBONamespace>GAZ</oboInOwl:hasOBONamespace>
        <oboInOwl:id>GAZ:00176003</oboInOwl:id>
        <rdfs:label>Al Jazeera Al Khadraa</rdfs:label>
    </owl:NamedIndividual>
    


    <!-- http://purl.obolibrary.org/obo/GAZ_00176005 -->

    <owl:NamedIndividual rdf:about="http://purl.obolibrary.org/obo/GAZ_00176005">
        <obo:RO_0001025 rdf:resource="http://purl.obolibrary.org/obo/GAZ_00007862"/>
        <obo:IAO_0000115>An island in the northern Gulf of Aqaba off the shore of Egypt&apos;s eastern Sinai Peninsula.</obo:IAO_0000115>
        <oboInOwl:hasOBONamespace>GAZ</oboInOwl:hasOBONamespace>
        <oboInOwl:id>GAZ:00176005</oboInOwl:id>
        <rdfs:label>Pharaoh&apos;s Island</rdfs:label>
    </owl:NamedIndividual>
    


    <!-- http://purl.obolibrary.org/obo/GAZ_00176006 -->

    <owl:NamedIndividual rdf:about="http://purl.obolibrary.org/obo/GAZ_00176006">
        <obo:RO_0001025 rdf:resource="http://purl.obolibrary.org/obo/GAZ_00002456"/>
        <obo:RO_0001025 rdf:resource="http://purl.obolibrary.org/obo/GAZ_00010398"/>
        <obo:IAO_0000115>An island off the coast of Saudi Arabia.</obo:IAO_0000115>
        <oboInOwl:hasOBONamespace>GAZ</oboInOwl:hasOBONamespace>
        <oboInOwl:id>GAZ:00176006</oboInOwl:id>
        <rdfs:label>Saso Island</rdfs:label>
    </owl:NamedIndividual>
    


    <!-- http://purl.obolibrary.org/obo/GAZ_00193804 -->

    <owl:NamedIndividual rdf:about="http://purl.obolibrary.org/obo/GAZ_00193804">
        <obo:RO_0001025 rdf:resource="http://purl.obolibrary.org/obo/GAZ_00007862"/>
        <obo:IAO_0000115>A protected area located on the Red Sea south of Eilat.</obo:IAO_0000115>
        <oboInOwl:hasOBONamespace>GAZ</oboInOwl:hasOBONamespace>
        <oboInOwl:id>GAZ:00193804</oboInOwl:id>
        <rdfs:label>Coral Beach Nature Reserve</rdfs:label>
    </owl:NamedIndividual>
    


    <!-- http://purl.obolibrary.org/obo/GAZ_00193987 -->

    <owl:NamedIndividual rdf:about="http://purl.obolibrary.org/obo/GAZ_00193987">
        <obo:IAO_0000115>A drainage canal. This canal is 560 km in length/ It runs southeast from Al Mahmudiya near Baghdad down the right bank of the Shatt Al Gharraf and crosses the Euphrates just east of Nasiriya, burrowing beneath the riverbed in three large pipes. It then skirts round the southwestern edge of Haur Al Hammar, crosses the southeast corner of the haur (between raised embankments), and finally joins up with the man-made Shatt Al Basrah canal which links the southeast corner of Haur Al Hammar to the head of the Gulf via Khawr Al Zubair. Constructed 1950s-to-1992-12.</obo:IAO_0000115>
        <oboInOwl:hasOBONamespace>GAZ</oboInOwl:hasOBONamespace>
        <oboInOwl:id>GAZ:00193987</oboInOwl:id>
        <rdfs:label>Main Outfall Drain</rdfs:label>
    </owl:NamedIndividual>
    


    <!-- http://purl.obolibrary.org/obo/GAZ_00246729 -->

    <owl:NamedIndividual rdf:about="http://purl.obolibrary.org/obo/GAZ_00246729">
        <obo:RO_0001025 rdf:resource="http://purl.obolibrary.org/obo/GAZ_00006937"/>
        <obo:IAO_0000115>A bay. Located at the northeast corner of the main island of Bahrain, almost surrounded by the capital city Manama.</obo:IAO_0000115>
        <oboInOwl:hasOBONamespace>GAZ</oboInOwl:hasOBONamespace>
        <oboInOwl:id>GAZ:00246729</oboInOwl:id>
        <rdfs:label>Tubli Bay</rdfs:label>
    </owl:NamedIndividual>
    


    <!-- http://purl.obolibrary.org/obo/GAZ_00246730 -->

    <owl:NamedIndividual rdf:about="http://purl.obolibrary.org/obo/GAZ_00246730">
        <obo:RO_0001025 rdf:resource="http://purl.obolibrary.org/obo/GAZ_00006937"/>
        <obo:IAO_0000115>An artificial lake. Located in the north-central part of the main island of Bahrain. It was created by the excavation of sand from a large pit, and is fed by seepage from underground sources and by run-off from adjacent irrigated land.</obo:IAO_0000115>
        <oboInOwl:hasOBONamespace>GAZ</oboInOwl:hasOBONamespace>
        <oboInOwl:id>GAZ:00246730</oboInOwl:id>
        <rdfs:label>Lawzi Lake</rdfs:label>
    </owl:NamedIndividual>
    


    <!-- http://purl.obolibrary.org/obo/GAZ_00246731 -->

    <owl:NamedIndividual rdf:about="http://purl.obolibrary.org/obo/GAZ_00246731">
        <obo:RO_0001025 rdf:resource="http://purl.obolibrary.org/obo/GAZ_00006937"/>
        <obo:IAO_0000115>A protected area on the SW coast of Bahrain. The site comprises a long stretch of sheltered sandy beach backed by low sand dunes and an adjacent small area of inter-tidal mudflats and sand flats.</obo:IAO_0000115>
        <oboInOwl:hasOBONamespace>GAZ</oboInOwl:hasOBONamespace>
        <oboInOwl:id>GAZ:00246731</oboInOwl:id>
        <rdfs:label>Mumtalah</rdfs:label>
    </owl:NamedIndividual>
    


    <!-- http://purl.obolibrary.org/obo/GAZ_00246732 -->

    <owl:NamedIndividual rdf:about="http://purl.obolibrary.org/obo/GAZ_00246732">
        <obo:RO_0001025 rdf:resource="http://purl.obolibrary.org/obo/GAZ_00006937"/>
        <obo:IAO_0000115>A large area of relatively undisturbed inter-tidal mudflats located on the SE coast of Bahrain.</obo:IAO_0000115>
        <oboInOwl:hasOBONamespace>GAZ</oboInOwl:hasOBONamespace>
        <oboInOwl:id>GAZ:00246732</oboInOwl:id>
        <rdfs:label>Ras Hayan</rdfs:label>
    </owl:NamedIndividual>
    


    <!-- http://purl.obolibrary.org/obo/GAZ_00248005 -->

    <owl:NamedIndividual rdf:about="http://purl.obolibrary.org/obo/GAZ_00248005">
        <obo:RO_0001025 rdf:resource="http://purl.obolibrary.org/obo/GAZ_00002456"/>
        <obo:IAO_0000115>An island offshore Al Ghardaqah.</obo:IAO_0000115>
        <oboInOwl:hasOBONamespace>GAZ</oboInOwl:hasOBONamespace>
        <oboInOwl:id>GAZ:00248005</oboInOwl:id>
        <rdfs:label>Abu Minciar Island</rdfs:label>
    </owl:NamedIndividual>
    


    <!-- http://purl.obolibrary.org/obo/GAZ_00248006 -->

    <owl:NamedIndividual rdf:about="http://purl.obolibrary.org/obo/GAZ_00248006">
        <obo:RO_0001025 rdf:resource="http://purl.obolibrary.org/obo/GAZ_00002456"/>
        <obo:IAO_0000115>An island offshore Port Sataga.</obo:IAO_0000115>
        <oboInOwl:hasOBONamespace>GAZ</oboInOwl:hasOBONamespace>
        <oboInOwl:id>GAZ:00248006</oboInOwl:id>
        <rdfs:label>Safaga Island</rdfs:label>
    </owl:NamedIndividual>
    


    <!-- http://purl.obolibrary.org/obo/GAZ_00248007 -->

    <owl:NamedIndividual rdf:about="http://purl.obolibrary.org/obo/GAZ_00248007">
        <obo:RO_0001025 rdf:resource="http://purl.obolibrary.org/obo/GAZ_00002456"/>
        <obo:IAO_0000115>An island.</obo:IAO_0000115>
        <oboInOwl:hasOBONamespace>GAZ</oboInOwl:hasOBONamespace>
        <oboInOwl:id>GAZ:00248007</oboInOwl:id>
        <rdfs:label>Jazirat Wadi Jimal</rdfs:label>
    </owl:NamedIndividual>
    


    <!-- http://purl.obolibrary.org/obo/GAZ_00248023 -->

    <owl:NamedIndividual rdf:about="http://purl.obolibrary.org/obo/GAZ_00248023">
        <obo:RO_0001025 rdf:resource="http://purl.obolibrary.org/obo/GAZ_00005295"/>
        <obo:IAO_0000115>An island.</obo:IAO_0000115>
        <oboInOwl:hasOBONamespace>GAZ</oboInOwl:hasOBONamespace>
        <oboInOwl:id>GAZ:00248023</oboInOwl:id>
        <rdfs:label>Sir Bani Yas</rdfs:label>
    </owl:NamedIndividual>
    


    <!-- http://purl.obolibrary.org/obo/GAZ_00248024 -->

    <owl:NamedIndividual rdf:about="http://purl.obolibrary.org/obo/GAZ_00248024">
        <obo:RO_0001025 rdf:resource="http://purl.obolibrary.org/obo/GAZ_00005295"/>
        <obo:IAO_0000115>A channel.</obo:IAO_0000115>
        <oboInOwl:hasOBONamespace>GAZ</oboInOwl:hasOBONamespace>
        <oboInOwl:id>GAZ:00248024</oboInOwl:id>
        <rdfs:label>Khawr al Bazm</rdfs:label>
    </owl:NamedIndividual>
    


    <!-- http://purl.obolibrary.org/obo/GAZ_00248025 -->

    <owl:NamedIndividual rdf:about="http://purl.obolibrary.org/obo/GAZ_00248025">
        <obo:RO_0001025 rdf:resource="http://purl.obolibrary.org/obo/GAZ_00005295"/>
        <obo:IAO_0000115>An island.</obo:IAO_0000115>
        <oboInOwl:hasOBONamespace>GAZ</oboInOwl:hasOBONamespace>
        <oboInOwl:id>GAZ:00248025</oboInOwl:id>
        <rdfs:label>Bu Khushayshah</rdfs:label>
    </owl:NamedIndividual>
    


    <!-- http://purl.obolibrary.org/obo/GAZ_00248026 -->

    <owl:NamedIndividual rdf:about="http://purl.obolibrary.org/obo/GAZ_00248026">
        <obo:RO_0001025 rdf:resource="http://purl.obolibrary.org/obo/GAZ_00005295"/>
        <obo:IAO_0000115>An island.</obo:IAO_0000115>
        <oboInOwl:hasOBONamespace>GAZ</oboInOwl:hasOBONamespace>
        <oboInOwl:id>GAZ:00248026</oboInOwl:id>
        <rdfs:label>Al Futaysi</rdfs:label>
    </owl:NamedIndividual>
    


    <!-- http://purl.obolibrary.org/obo/GAZ_00248027 -->

    <owl:NamedIndividual rdf:about="http://purl.obolibrary.org/obo/GAZ_00248027">
        <obo:RO_0001025 rdf:resource="http://purl.obolibrary.org/obo/GAZ_00005295"/>
        <obo:IAO_0000115>An island.</obo:IAO_0000115>
        <oboInOwl:hasOBONamespace>GAZ</oboInOwl:hasOBONamespace>
        <oboInOwl:id>GAZ:00248027</oboInOwl:id>
        <rdfs:label>Halat al Bahrani</rdfs:label>
    </owl:NamedIndividual>
    


    <!-- http://purl.obolibrary.org/obo/GAZ_00248028 -->

    <owl:NamedIndividual rdf:about="http://purl.obolibrary.org/obo/GAZ_00248028">
        <obo:RO_0001025 rdf:resource="http://purl.obolibrary.org/obo/GAZ_00005295"/>
        <obo:IAO_0000115>An island.</obo:IAO_0000115>
        <oboInOwl:hasOBONamespace>GAZ</oboInOwl:hasOBONamespace>
        <oboInOwl:id>GAZ:00248028</oboInOwl:id>
        <rdfs:label>&apos;Ushsh</rdfs:label>
    </owl:NamedIndividual>
    


    <!-- http://purl.obolibrary.org/obo/GAZ_00248029 -->

    <owl:NamedIndividual rdf:about="http://purl.obolibrary.org/obo/GAZ_00248029">
        <obo:RO_0001025 rdf:resource="http://purl.obolibrary.org/obo/GAZ_00005295"/>
        <obo:IAO_0000115>An island.</obo:IAO_0000115>
        <oboInOwl:hasOBONamespace>GAZ</oboInOwl:hasOBONamespace>
        <oboInOwl:id>GAZ:00248029</oboInOwl:id>
        <rdfs:label>Umm &apos;Amim</rdfs:label>
    </owl:NamedIndividual>
    


    <!-- http://purl.obolibrary.org/obo/GAZ_00248030 -->

    <owl:NamedIndividual rdf:about="http://purl.obolibrary.org/obo/GAZ_00248030">
        <obo:RO_0001025 rdf:resource="http://purl.obolibrary.org/obo/GAZ_00005295"/>
        <obo:IAO_0000115>An island.</obo:IAO_0000115>
        <oboInOwl:hasOBONamespace>GAZ</oboInOwl:hasOBONamespace>
        <oboInOwl:id>GAZ:00248030</oboInOwl:id>
        <rdfs:label>Jananah</rdfs:label>
    </owl:NamedIndividual>
    


    <!-- http://purl.obolibrary.org/obo/GAZ_00248031 -->

    <owl:NamedIndividual rdf:about="http://purl.obolibrary.org/obo/GAZ_00248031">
        <rdf:type rdf:resource="http://purl.obolibrary.org/obo/ENVO_00000167"/>
        <obo:RO_0001025 rdf:resource="http://purl.obolibrary.org/obo/GAZ_00005295"/>
        <obo:IAO_0000115>A shoal.</obo:IAO_0000115>
        <oboInOwl:hasOBONamespace>GAZ</oboInOwl:hasOBONamespace>
        <oboInOwl:id>GAZ:00248031</oboInOwl:id>
        <rdfs:label>Bu Tinah</rdfs:label>
    </owl:NamedIndividual>
    


    <!-- http://purl.obolibrary.org/obo/GAZ_00248035 -->

    <owl:NamedIndividual rdf:about="http://purl.obolibrary.org/obo/GAZ_00248035">
        <obo:RO_0001025 rdf:resource="http://purl.obolibrary.org/obo/GAZ_00005295"/>
        <obo:IAO_0000115>An island. A satellite of Sir Bani Yas.</obo:IAO_0000115>
        <oboInOwl:hasOBONamespace>GAZ</oboInOwl:hasOBONamespace>
        <oboInOwl:id>GAZ:00248035</oboInOwl:id>
        <rdfs:label>Umm Qassar</rdfs:label>
    </owl:NamedIndividual>
    


    <!-- http://purl.obolibrary.org/obo/GAZ_00248036 -->

    <owl:NamedIndividual rdf:about="http://purl.obolibrary.org/obo/GAZ_00248036">
        <obo:RO_0001025 rdf:resource="http://purl.obolibrary.org/obo/GAZ_00005295"/>
        <oboInOwl:hasOBONamespace>GAZ</oboInOwl:hasOBONamespace>
        <oboInOwl:id>GAZ:00248036</oboInOwl:id>
        <rdfs:label>Umm al Kirkum</rdfs:label>
    </owl:NamedIndividual>
    


    <!-- http://purl.obolibrary.org/obo/GAZ_00248037 -->

    <owl:NamedIndividual rdf:about="http://purl.obolibrary.org/obo/GAZ_00248037">
        <obo:RO_0001025 rdf:resource="http://purl.obolibrary.org/obo/GAZ_00005295"/>
        <oboInOwl:hasOBONamespace>GAZ</oboInOwl:hasOBONamespace>
        <oboInOwl:id>GAZ:00248037</oboInOwl:id>
        <rdfs:label>Ghasha</rdfs:label>
    </owl:NamedIndividual>
    


    <!-- http://purl.obolibrary.org/obo/GAZ_00248038 -->

    <owl:NamedIndividual rdf:about="http://purl.obolibrary.org/obo/GAZ_00248038">
        <obo:RO_0001025 rdf:resource="http://purl.obolibrary.org/obo/GAZ_00005295"/>
        <obo:IAO_0000115>An island.</obo:IAO_0000115>
        <oboInOwl:hasOBONamespace>GAZ</oboInOwl:hasOBONamespace>
        <oboInOwl:id>GAZ:00248038</oboInOwl:id>
        <rdfs:label>Al Yasat</rdfs:label>
    </owl:NamedIndividual>
    


    <!-- http://purl.obolibrary.org/obo/GAZ_00248039 -->

    <owl:NamedIndividual rdf:about="http://purl.obolibrary.org/obo/GAZ_00248039">
        <obo:RO_0001025 rdf:resource="http://purl.obolibrary.org/obo/GAZ_00005295"/>
        <obo:IAO_0000115>An island.</obo:IAO_0000115>
        <oboInOwl:hasOBONamespace>GAZ</oboInOwl:hasOBONamespace>
        <oboInOwl:id>GAZ:00248039</oboInOwl:id>
        <rdfs:label>Al Yasat as Sufla</rdfs:label>
    </owl:NamedIndividual>
    


    <!-- http://purl.obolibrary.org/obo/GAZ_00248040 -->

    <owl:NamedIndividual rdf:about="http://purl.obolibrary.org/obo/GAZ_00248040">
        <obo:RO_0001025 rdf:resource="http://purl.obolibrary.org/obo/GAZ_00005295"/>
        <obo:IAO_0000115>An island.</obo:IAO_0000115>
        <oboInOwl:hasOBONamespace>GAZ</oboInOwl:hasOBONamespace>
        <oboInOwl:id>GAZ:00248040</oboInOwl:id>
        <rdfs:label>Al Yasat al &apos;Ulya</rdfs:label>
    </owl:NamedIndividual>
    


    <!-- http://purl.obolibrary.org/obo/GAZ_00248041 -->

    <owl:NamedIndividual rdf:about="http://purl.obolibrary.org/obo/GAZ_00248041">
        <obo:RO_0001025 rdf:resource="http://purl.obolibrary.org/obo/GAZ_00005295"/>
        <obo:IAO_0000115>An island.</obo:IAO_0000115>
        <oboInOwl:hasOBONamespace>GAZ</oboInOwl:hasOBONamespace>
        <oboInOwl:id>GAZ:00248041</oboInOwl:id>
        <rdfs:label>Ghaghah</rdfs:label>
    </owl:NamedIndividual>
    


    <!-- http://purl.obolibrary.org/obo/GAZ_00248042 -->

    <owl:NamedIndividual rdf:about="http://purl.obolibrary.org/obo/GAZ_00248042">
        <obo:RO_0001025 rdf:resource="http://purl.obolibrary.org/obo/GAZ_00005295"/>
        <obo:IAO_0000115>An island.</obo:IAO_0000115>
        <oboInOwl:hasOBONamespace>GAZ</oboInOwl:hasOBONamespace>
        <oboInOwl:id>GAZ:00248042</oboInOwl:id>
        <rdfs:label>Umm al Hatab</rdfs:label>
    </owl:NamedIndividual>
    


    <!-- http://purl.obolibrary.org/obo/GAZ_00248043 -->

    <owl:NamedIndividual rdf:about="http://purl.obolibrary.org/obo/GAZ_00248043">
        <obo:RO_0001025 rdf:resource="http://purl.obolibrary.org/obo/GAZ_00005295"/>
        <obo:IAO_0000115>An island.</obo:IAO_0000115>
        <oboInOwl:hasOBONamespace>GAZ</oboInOwl:hasOBONamespace>
        <oboInOwl:id>GAZ:00248043</oboInOwl:id>
        <rdfs:label>Makasib</rdfs:label>
    </owl:NamedIndividual>
    


    <!-- http://purl.obolibrary.org/obo/GAZ_00248044 -->

    <owl:NamedIndividual rdf:about="http://purl.obolibrary.org/obo/GAZ_00248044">
        <obo:RO_0001025 rdf:resource="http://purl.obolibrary.org/obo/GAZ_00005295"/>
        <obo:IAO_0000115>An island.</obo:IAO_0000115>
        <oboInOwl:hasOBONamespace>GAZ</oboInOwl:hasOBONamespace>
        <oboInOwl:id>GAZ:00248044</oboInOwl:id>
        <rdfs:label>Al Qaffay</rdfs:label>
    </owl:NamedIndividual>
    


    <!-- http://purl.obolibrary.org/obo/GAZ_00248045 -->

    <owl:NamedIndividual rdf:about="http://purl.obolibrary.org/obo/GAZ_00248045">
        <obo:RO_0001025 rdf:resource="http://purl.obolibrary.org/obo/GAZ_00005295"/>
        <obo:IAO_0000115>An island.</obo:IAO_0000115>
        <oboInOwl:hasOBONamespace>GAZ</oboInOwl:hasOBONamespace>
        <oboInOwl:id>GAZ:00248045</oboInOwl:id>
        <rdfs:label>Muhammaliyah</rdfs:label>
    </owl:NamedIndividual>
    


    <!-- http://purl.obolibrary.org/obo/GAZ_00248046 -->

    <owl:NamedIndividual rdf:about="http://purl.obolibrary.org/obo/GAZ_00248046">
        <obo:RO_0001025 rdf:resource="http://purl.obolibrary.org/obo/GAZ_00005295"/>
        <obo:IAO_0000115>An offshore island.</obo:IAO_0000115>
        <oboInOwl:hasOBONamespace>GAZ</oboInOwl:hasOBONamespace>
        <oboInOwl:id>GAZ:00248046</oboInOwl:id>
        <rdfs:label>Dayyinah</rdfs:label>
    </owl:NamedIndividual>
    


    <!-- http://purl.obolibrary.org/obo/GAZ_00248047 -->

    <owl:NamedIndividual rdf:about="http://purl.obolibrary.org/obo/GAZ_00248047">
        <obo:RO_0001025 rdf:resource="http://purl.obolibrary.org/obo/GAZ_00005295"/>
        <obo:IAO_0000115>An offshore island.</obo:IAO_0000115>
        <oboInOwl:hasOBONamespace>GAZ</oboInOwl:hasOBONamespace>
        <oboInOwl:id>GAZ:00248047</oboInOwl:id>
        <rdfs:label>Qarnayn</rdfs:label>
    </owl:NamedIndividual>
    


    <!-- http://purl.obolibrary.org/obo/GAZ_00248048 -->

    <owl:NamedIndividual rdf:about="http://purl.obolibrary.org/obo/GAZ_00248048">
        <obo:RO_0001025 rdf:resource="http://purl.obolibrary.org/obo/GAZ_00005295"/>
        <obo:IAO_0000115>An offshore island.</obo:IAO_0000115>
        <oboInOwl:hasOBONamespace>GAZ</oboInOwl:hasOBONamespace>
        <oboInOwl:id>GAZ:00248048</oboInOwl:id>
        <rdfs:label>Arzanah</rdfs:label>
    </owl:NamedIndividual>
    


    <!-- http://purl.obolibrary.org/obo/GAZ_00248049 -->

    <owl:NamedIndividual rdf:about="http://purl.obolibrary.org/obo/GAZ_00248049">
        <obo:RO_0001025 rdf:resource="http://purl.obolibrary.org/obo/GAZ_00005295"/>
        <obo:IAO_0000115>An offshore island.</obo:IAO_0000115>
        <oboInOwl:hasOBONamespace>GAZ</oboInOwl:hasOBONamespace>
        <oboInOwl:id>GAZ:00248049</oboInOwl:id>
        <rdfs:label>Zirkuh</rdfs:label>
    </owl:NamedIndividual>
    


    <!-- http://purl.obolibrary.org/obo/GAZ_00248050 -->

    <owl:NamedIndividual rdf:about="http://purl.obolibrary.org/obo/GAZ_00248050">
        <obo:RO_0001025 rdf:resource="http://purl.obolibrary.org/obo/GAZ_00005295"/>
        <obo:IAO_0000115>An island off eastern Abu Dhabi.</obo:IAO_0000115>
        <oboInOwl:hasOBONamespace>GAZ</oboInOwl:hasOBONamespace>
        <oboInOwl:id>GAZ:00248050</oboInOwl:id>
        <rdfs:label>As Sa&apos;diyat</rdfs:label>
    </owl:NamedIndividual>
    


    <!-- http://purl.obolibrary.org/obo/GAZ_00248051 -->

    <owl:NamedIndividual rdf:about="http://purl.obolibrary.org/obo/GAZ_00248051">
        <obo:RO_0001025 rdf:resource="http://purl.obolibrary.org/obo/GAZ_00005295"/>
        <obo:IAO_0000115>An island off eastern Abu Dhabi.</obo:IAO_0000115>
        <oboInOwl:hasOBONamespace>GAZ</oboInOwl:hasOBONamespace>
        <oboInOwl:id>GAZ:00248051</oboInOwl:id>
        <rdfs:label>Jazirat Ramhan</rdfs:label>
    </owl:NamedIndividual>
    


    <!-- http://purl.obolibrary.org/obo/GAZ_00248052 -->

    <owl:NamedIndividual rdf:about="http://purl.obolibrary.org/obo/GAZ_00248052">
        <obo:RO_0001025 rdf:resource="http://purl.obolibrary.org/obo/GAZ_00005295"/>
        <obo:IAO_0000115>An island off eastern Abu Dhabi.</obo:IAO_0000115>
        <oboInOwl:hasOBONamespace>GAZ</oboInOwl:hasOBONamespace>
        <oboInOwl:id>GAZ:00248052</oboInOwl:id>
        <rdfs:label>Bu Hayl</rdfs:label>
    </owl:NamedIndividual>
    


    <!-- http://purl.obolibrary.org/obo/GAZ_00248053 -->

    <owl:NamedIndividual rdf:about="http://purl.obolibrary.org/obo/GAZ_00248053">
        <obo:RO_0001025 rdf:resource="http://purl.obolibrary.org/obo/GAZ_00005295"/>
        <obo:IAO_0000115>An island off eastern Abu Dhabi.</obo:IAO_0000115>
        <oboInOwl:hasOBONamespace>GAZ</oboInOwl:hasOBONamespace>
        <oboInOwl:id>GAZ:00248053</oboInOwl:id>
        <rdfs:label>Hayl</rdfs:label>
    </owl:NamedIndividual>
    


    <!-- http://purl.obolibrary.org/obo/GAZ_00248054 -->

    <owl:NamedIndividual rdf:about="http://purl.obolibrary.org/obo/GAZ_00248054">
        <obo:RO_0001025 rdf:resource="http://purl.obolibrary.org/obo/GAZ_00005295"/>
        <obo:IAO_0000115>An island off eastern Abu Dhabi.</obo:IAO_0000115>
        <oboInOwl:hasOBONamespace>GAZ</oboInOwl:hasOBONamespace>
        <oboInOwl:id>GAZ:00248054</oboInOwl:id>
        <rdfs:label>Jazirat Ra&apos;s Ghurab</rdfs:label>
    </owl:NamedIndividual>
    


    <!-- http://purl.obolibrary.org/obo/GAZ_00248055 -->

    <owl:NamedIndividual rdf:about="http://purl.obolibrary.org/obo/GAZ_00248055">
        <obo:RO_0001025 rdf:resource="http://purl.obolibrary.org/obo/GAZ_00005295"/>
        <obo:IAO_0000115>An island off eastern Abu Dhabi.</obo:IAO_0000115>
        <oboInOwl:hasOBONamespace>GAZ</oboInOwl:hasOBONamespace>
        <oboInOwl:id>GAZ:00248055</oboInOwl:id>
        <rdfs:label>Ra&apos;s Ghanadah</rdfs:label>
    </owl:NamedIndividual>
    


    <!-- http://purl.obolibrary.org/obo/GAZ_00248057 -->

    <owl:NamedIndividual rdf:about="http://purl.obolibrary.org/obo/GAZ_00248057">
        <obo:RO_0001025 rdf:resource="http://purl.obolibrary.org/obo/GAZ_00005295"/>
        <obo:IAO_0000115>An island. Located in the Persian Gulf, 75 km from the mainland coast of Abu Dhabi, Abu Dhabi Emirate.</obo:IAO_0000115>
        <oboInOwl:hasOBONamespace>GAZ</oboInOwl:hasOBONamespace>
        <oboInOwl:id>GAZ:00248057</oboInOwl:id>
        <rdfs:label>Sir Bu Nu&apos;ayr</rdfs:label>
    </owl:NamedIndividual>
    


    <!-- http://purl.obolibrary.org/obo/GAZ_00248061 -->

    <owl:NamedIndividual rdf:about="http://purl.obolibrary.org/obo/GAZ_00248061">
        <rdf:type rdf:resource="http://purl.obolibrary.org/obo/ENVO_00000475"/>
        <obo:RO_0001025 rdf:resource="http://purl.obolibrary.org/obo/GAZ_00005295"/>
        <obo:IAO_0000115>A tidal creek. An arm of Khor Zawra.</obo:IAO_0000115>
        <oboInOwl:hasOBONamespace>GAZ</oboInOwl:hasOBONamespace>
        <oboInOwl:id>GAZ:00248061</oboInOwl:id>
        <rdfs:label>Khor Zawra</rdfs:label>
    </owl:NamedIndividual>
    


    <!-- http://purl.obolibrary.org/obo/GAZ_00248062 -->

    <owl:NamedIndividual rdf:about="http://purl.obolibrary.org/obo/GAZ_00248062">
        <obo:RO_0001025 rdf:resource="http://purl.obolibrary.org/obo/GAZ_00005295"/>
        <obo:IAO_0000115>A wetland located on the Arabian Gulf coast east of Umm al Qaiwain city and on the landward (southeast) side of Sinaiya Island, Umm al Qaiwain Emirate. It comprises a vast complex of lagoons, 20 km long by an average of 4 km wide, with about 25 low sandy islands, each of less than 50 ha in extent except for the three mangrove-covered round islands of Jazirat al Ghubbah (Ghallah), which are between one and two km in diameter.</obo:IAO_0000115>
        <oboInOwl:hasOBONamespace>GAZ</oboInOwl:hasOBONamespace>
        <oboInOwl:id>GAZ:00248062</oboInOwl:id>
        <rdfs:label>Khor al Beidah</rdfs:label>
    </owl:NamedIndividual>
    


    <!-- http://purl.obolibrary.org/obo/GAZ_00248063 -->

    <owl:NamedIndividual rdf:about="http://purl.obolibrary.org/obo/GAZ_00248063">
        <obo:RO_0001025 rdf:resource="http://purl.obolibrary.org/obo/GAZ_00005295"/>
        <obo:IAO_0000115>An island.</obo:IAO_0000115>
        <oboInOwl:hasOBONamespace>GAZ</oboInOwl:hasOBONamespace>
        <oboInOwl:id>GAZ:00248063</oboInOwl:id>
        <rdfs:label>Jazirat as Siniyah</rdfs:label>
    </owl:NamedIndividual>
    


    <!-- http://purl.obolibrary.org/obo/GAZ_00248064 -->

    <owl:NamedIndividual rdf:about="http://purl.obolibrary.org/obo/GAZ_00248064">
        <obo:RO_0001025 rdf:resource="http://purl.obolibrary.org/obo/GAZ_00005295"/>
        <obo:IAO_0000115>An island.</obo:IAO_0000115>
        <oboInOwl:hasOBONamespace>GAZ</oboInOwl:hasOBONamespace>
        <oboInOwl:id>GAZ:00248064</oboInOwl:id>
        <rdfs:label>Jazirat al Ghallah</rdfs:label>
    </owl:NamedIndividual>
    


    <!-- http://purl.obolibrary.org/obo/GAZ_00248065 -->

    <owl:NamedIndividual rdf:about="http://purl.obolibrary.org/obo/GAZ_00248065">
        <obo:RO_0001025 rdf:resource="http://purl.obolibrary.org/obo/GAZ_00248062"/>
        <obo:IAO_0000115>Three mangrove-covered islands.</obo:IAO_0000115>
        <oboInOwl:hasOBONamespace>GAZ</oboInOwl:hasOBONamespace>
        <oboInOwl:id>GAZ:00248065</oboInOwl:id>
        <rdfs:label>Jazirat al Ghubbah</rdfs:label>
    </owl:NamedIndividual>
    


    <!-- http://purl.obolibrary.org/obo/GAZ_00248066 -->

    <owl:NamedIndividual rdf:about="http://purl.obolibrary.org/obo/GAZ_00248066">
        <obo:RO_0001025 rdf:resource="http://purl.obolibrary.org/obo/GAZ_00248062"/>
        <obo:IAO_0000115>The southwestern portion of the lagoons of Khor al Beidah.</obo:IAO_0000115>
        <oboInOwl:hasOBONamespace>GAZ</oboInOwl:hasOBONamespace>
        <oboInOwl:id>GAZ:00248066</oboInOwl:id>
        <rdfs:label>Khor Umm al Qaiwain</rdfs:label>
    </owl:NamedIndividual>
    


    <!-- http://purl.obolibrary.org/obo/GAZ_00248067 -->

    <owl:NamedIndividual rdf:about="http://purl.obolibrary.org/obo/GAZ_00248067">
        <obo:RO_0001025 rdf:resource="http://purl.obolibrary.org/obo/GAZ_00005295"/>
        <obo:IAO_0000115>A complex of shallow tidal lagoons and inter-tidal mudflats on the Gulf coast, with areas of higher ground covered with halophytic scrub.</obo:IAO_0000115>
        <oboInOwl:hasOBONamespace>GAZ</oboInOwl:hasOBONamespace>
        <oboInOwl:id>GAZ:00248067</oboInOwl:id>
        <rdfs:label>Al Jazeerah Khor</rdfs:label>
    </owl:NamedIndividual>
    


    <!-- http://purl.obolibrary.org/obo/GAZ_00248068 -->

    <owl:NamedIndividual rdf:about="http://purl.obolibrary.org/obo/GAZ_00248068">
        <obo:RO_0001025 rdf:resource="http://purl.obolibrary.org/obo/GAZ_00005295"/>
        <obo:IAO_0000115>An island. Off the W side of the Musandam Peninsula.</obo:IAO_0000115>
        <oboInOwl:hasOBONamespace>GAZ</oboInOwl:hasOBONamespace>
        <oboInOwl:id>GAZ:00248068</oboInOwl:id>
        <rdfs:label>Jazirat Hulaylah</rdfs:label>
    </owl:NamedIndividual>
    


    <!-- http://purl.obolibrary.org/obo/GAZ_00248069 -->

    <owl:NamedIndividual rdf:about="http://purl.obolibrary.org/obo/GAZ_00248069">
        <obo:RO_0001025 rdf:resource="http://purl.obolibrary.org/obo/GAZ_00005295"/>
        <obo:IAO_0000115>An island.</obo:IAO_0000115>
        <oboInOwl:hasOBONamespace>GAZ</oboInOwl:hasOBONamespace>
        <oboInOwl:id>GAZ:00248069</oboInOwl:id>
        <rdfs:label>Jazirat al Hamra&apos;</rdfs:label>
    </owl:NamedIndividual>
    


    <!-- http://purl.obolibrary.org/obo/GAZ_00248070 -->

    <owl:NamedIndividual rdf:about="http://purl.obolibrary.org/obo/GAZ_00248070">
        <obo:RO_0001025 rdf:resource="http://purl.obolibrary.org/obo/GAZ_00005295"/>
        <obo:IAO_0000115>An island.</obo:IAO_0000115>
        <oboInOwl:hasOBONamespace>GAZ</oboInOwl:hasOBONamespace>
        <oboInOwl:id>GAZ:00248070</oboInOwl:id>
        <rdfs:label>Jazirat Qurmah</rdfs:label>
    </owl:NamedIndividual>
    


    <!-- http://purl.obolibrary.org/obo/GAZ_00248071 -->

    <owl:NamedIndividual rdf:about="http://purl.obolibrary.org/obo/GAZ_00248071">
        <obo:RO_0001025 rdf:resource="http://purl.obolibrary.org/obo/GAZ_00005295"/>
        <obo:IAO_0000115>A bay on the east coast of the UAE in Fujairah and Sharjah Emirates, and straddling the border with Oman.</obo:IAO_0000115>
        <oboInOwl:hasOBONamespace>GAZ</oboInOwl:hasOBONamespace>
        <oboInOwl:id>GAZ:00248071</oboInOwl:id>
        <rdfs:label>Dawhat Diba</rdfs:label>
    </owl:NamedIndividual>
    


    <!-- http://purl.obolibrary.org/obo/GAZ_00248075 -->

    <owl:NamedIndividual rdf:about="http://purl.obolibrary.org/obo/GAZ_00248075">
        <obo:RO_0001025 rdf:resource="http://purl.obolibrary.org/obo/GAZ_00005295"/>
        <obo:IAO_0000115>A tidal inlet. Khor Kalba is a small, shallow, tidal inlet with ramifying channels formed by the outlet of Wadi Rumh.</obo:IAO_0000115>
        <oboInOwl:hasOBONamespace>GAZ</oboInOwl:hasOBONamespace>
        <oboInOwl:id>GAZ:00248075</oboInOwl:id>
        <rdfs:label>Khor Kalba</rdfs:label>
    </owl:NamedIndividual>
    


    <!-- http://purl.obolibrary.org/obo/GAZ_00248111 -->

    <owl:NamedIndividual rdf:about="http://purl.obolibrary.org/obo/GAZ_00248111">
        <obo:RO_0001025 rdf:resource="http://purl.obolibrary.org/obo/GAZ_00002456"/>
        <obo:IAO_0000115>A bay.</obo:IAO_0000115>
        <oboInOwl:hasOBONamespace>GAZ</oboInOwl:hasOBONamespace>
        <oboInOwl:id>GAZ:00248111</oboInOwl:id>
        <rdfs:label>Mersa Mubarec</rdfs:label>
    </owl:NamedIndividual>
    


    <!-- http://purl.obolibrary.org/obo/GAZ_00248112 -->

    <owl:NamedIndividual rdf:about="http://purl.obolibrary.org/obo/GAZ_00248112">
        <obo:RO_0001025 rdf:resource="http://purl.obolibrary.org/obo/GAZ_00002456"/>
        <obo:IAO_0000115>An inlet.</obo:IAO_0000115>
        <oboInOwl:hasOBONamespace>GAZ</oboInOwl:hasOBONamespace>
        <oboInOwl:id>GAZ:00248112</oboInOwl:id>
        <rdfs:label>Mersa Deresa</rdfs:label>
    </owl:NamedIndividual>
    


    <!-- http://purl.obolibrary.org/obo/GAZ_00248117 -->

    <owl:NamedIndividual rdf:about="http://purl.obolibrary.org/obo/GAZ_00248117">
        <obo:RO_0001025 rdf:resource="http://purl.obolibrary.org/obo/GAZ_00002456"/>
        <obo:IAO_0000115>A bay.</obo:IAO_0000115>
        <oboInOwl:hasOBONamespace>GAZ</oboInOwl:hasOBONamespace>
        <oboInOwl:id>GAZ:00248117</oboInOwl:id>
        <rdfs:label>Assab Bahir Selat&apos;e</rdfs:label>
    </owl:NamedIndividual>
    


    <!-- http://purl.obolibrary.org/obo/GAZ_00248118 -->

    <owl:NamedIndividual rdf:about="http://purl.obolibrary.org/obo/GAZ_00248118">
        <obo:RO_0001025 rdf:resource="http://purl.obolibrary.org/obo/GAZ_00002456"/>
        <obo:RO_0001025 rdf:resource="http://purl.obolibrary.org/obo/GAZ_00248117"/>
        <obo:IAO_0000115>An island.</obo:IAO_0000115>
        <oboInOwl:hasOBONamespace>GAZ</oboInOwl:hasOBONamespace>
        <oboInOwl:id>GAZ:00248118</oboInOwl:id>
        <rdfs:label>Fatuma Deset</rdfs:label>
    </owl:NamedIndividual>
    


    <!-- http://purl.obolibrary.org/obo/GAZ_00250868 -->

    <owl:NamedIndividual rdf:about="http://purl.obolibrary.org/obo/GAZ_00250868">
        <obo:RO_0001025 rdf:resource="http://purl.obolibrary.org/obo/GAZ_00005295"/>
        <obo:IAO_0000115>A marine channel at the head of the Persian Gulf.</obo:IAO_0000115>
        <oboInOwl:hasOBONamespace>GAZ</oboInOwl:hasOBONamespace>
        <oboInOwl:id>GAZ:00250868</oboInOwl:id>
        <rdfs:label>Khor-al Amaya</rdfs:label>
    </owl:NamedIndividual>
    


    <!-- http://purl.obolibrary.org/obo/GAZ_00250869 -->

    <owl:NamedIndividual rdf:about="http://purl.obolibrary.org/obo/GAZ_00250869">
        <obo:RO_0001025 rdf:resource="http://purl.obolibrary.org/obo/GAZ_00005295"/>
        <obo:IAO_0000115>A marine channel at the head of the Persian Gulf.</obo:IAO_0000115>
        <oboInOwl:hasOBONamespace>GAZ</oboInOwl:hasOBONamespace>
        <oboInOwl:id>GAZ:00250869</oboInOwl:id>
        <rdfs:label>Khor Musa</rdfs:label>
    </owl:NamedIndividual>
    


    <!-- http://purl.obolibrary.org/obo/GAZ_00250909 -->

    <owl:NamedIndividual rdf:about="http://purl.obolibrary.org/obo/GAZ_00250909">
        <obo:RO_0001025 rdf:resource="http://purl.obolibrary.org/obo/GAZ_00005295"/>
        <obo:IAO_0000115>A small sandy island with fringing coral reefs in the northern Persian Gulf.</obo:IAO_0000115>
        <oboInOwl:hasOBONamespace>GAZ</oboInOwl:hasOBONamespace>
        <oboInOwl:id>GAZ:00250909</oboInOwl:id>
        <rdfs:label>Jazireh-ye Kharku</rdfs:label>
    </owl:NamedIndividual>
    


    <!-- http://purl.obolibrary.org/obo/GAZ_00250911 -->

    <owl:NamedIndividual rdf:about="http://purl.obolibrary.org/obo/GAZ_00250911">
        <obo:IAO_0000115>A river.</obo:IAO_0000115>
        <oboInOwl:hasOBONamespace>GAZ</oboInOwl:hasOBONamespace>
        <oboInOwl:id>GAZ:00250911</oboInOwl:id>
        <rdfs:label>Helleh Rud</rdfs:label>
    </owl:NamedIndividual>
    


    <!-- http://purl.obolibrary.org/obo/GAZ_00250912 -->

    <owl:NamedIndividual rdf:about="http://purl.obolibrary.org/obo/GAZ_00250912">
        <obo:RO_0001025 rdf:resource="http://purl.obolibrary.org/obo/GAZ_00250911"/>
        <obo:IAO_0000115>The delta of the Helleh River.</obo:IAO_0000115>
        <oboInOwl:hasOBONamespace>GAZ</oboInOwl:hasOBONamespace>
        <oboInOwl:id>GAZ:00250912</oboInOwl:id>
        <rdfs:label>Helleh Delta</rdfs:label>
    </owl:NamedIndividual>
    


    <!-- http://purl.obolibrary.org/obo/GAZ_00250913 -->

    <owl:NamedIndividual rdf:about="http://purl.obolibrary.org/obo/GAZ_00250913">
        <obo:RO_0001025 rdf:resource="http://purl.obolibrary.org/obo/GAZ_00005295"/>
        <obo:IAO_0000115>A shallow sea bay.</obo:IAO_0000115>
        <oboInOwl:hasOBONamespace>GAZ</oboInOwl:hasOBONamespace>
        <oboInOwl:id>GAZ:00250913</oboInOwl:id>
        <rdfs:label>Bushehr Bay</rdfs:label>
    </owl:NamedIndividual>
    


    <!-- http://purl.obolibrary.org/obo/GAZ_00250917 -->

    <owl:NamedIndividual rdf:about="http://purl.obolibrary.org/obo/GAZ_00250917">
        <obo:RO_0001025 rdf:resource="http://purl.obolibrary.org/obo/GAZ_00005295"/>
        <obo:IAO_0000115>A sandy inshore island. Located in the Persian Gulf about 40 km southeast of the Monde River Delta.</obo:IAO_0000115>
        <oboInOwl:hasOBONamespace>GAZ</oboInOwl:hasOBONamespace>
        <oboInOwl:id>GAZ:00250917</oboInOwl:id>
        <rdfs:label>Nakhilu Island</rdfs:label>
    </owl:NamedIndividual>
    


    <!-- http://purl.obolibrary.org/obo/GAZ_00250918 -->

    <owl:NamedIndividual rdf:about="http://purl.obolibrary.org/obo/GAZ_00250918">
        <obo:RO_0001025 rdf:resource="http://purl.obolibrary.org/obo/GAZ_00005295"/>
        <obo:IAO_0000115>A sandy inshore island. Located in the Persian Gulf about 40 km southeast of the Monde River Delta.</obo:IAO_0000115>
        <oboInOwl:hasOBONamespace>GAZ</oboInOwl:hasOBONamespace>
        <oboInOwl:id>GAZ:00250918</oboInOwl:id>
        <rdfs:label>Morghu Island</rdfs:label>
    </owl:NamedIndividual>
    


    <!-- http://purl.obolibrary.org/obo/GAZ_00250919 -->

    <owl:NamedIndividual rdf:about="http://purl.obolibrary.org/obo/GAZ_00250919">
        <obo:RO_0001025 rdf:resource="http://purl.obolibrary.org/obo/GAZ_00005295"/>
        <obo:IAO_0000115>A sandy inshore island. Located in the Persian Gulf about 40 km southeast of the Monde River Delta.</obo:IAO_0000115>
        <oboInOwl:hasOBONamespace>GAZ</oboInOwl:hasOBONamespace>
        <oboInOwl:id>GAZ:00250919</oboInOwl:id>
        <rdfs:label>Umm al Korm Island</rdfs:label>
    </owl:NamedIndividual>
    


    <!-- http://purl.obolibrary.org/obo/GAZ_00250920 -->

    <owl:NamedIndividual rdf:about="http://purl.obolibrary.org/obo/GAZ_00250920">
        <obo:RO_0001025 rdf:resource="http://purl.obolibrary.org/obo/GAZ_00005295"/>
        <obo:IAO_0000115>Two small rocky offshore islands in the south-central Persian Gulf, 45 km southwest of Bandar Lengeh.</obo:IAO_0000115>
        <oboInOwl:hasOBONamespace>GAZ</oboInOwl:hasOBONamespace>
        <oboInOwl:id>GAZ:00250920</oboInOwl:id>
        <rdfs:label>Faror Islands</rdfs:label>
    </owl:NamedIndividual>
    


    <!-- http://purl.obolibrary.org/obo/GAZ_00250921 -->

    <owl:NamedIndividual rdf:about="http://purl.obolibrary.org/obo/GAZ_00250921">
        <obo:RO_0001025 rdf:resource="http://purl.obolibrary.org/obo/GAZ_00250920"/>
        <obo:IAO_0000115>A protected area.</obo:IAO_0000115>
        <oboInOwl:hasOBONamespace>GAZ</oboInOwl:hasOBONamespace>
        <oboInOwl:id>GAZ:00250921</oboInOwl:id>
        <rdfs:label>Faror Protected Area</rdfs:label>
    </owl:NamedIndividual>
    


    <!-- http://purl.obolibrary.org/obo/GAZ_00250922 -->

    <owl:NamedIndividual rdf:about="http://purl.obolibrary.org/obo/GAZ_00250922">
        <obo:RO_0001025 rdf:resource="http://purl.obolibrary.org/obo/GAZ_00005295"/>
        <obo:IAO_0000115>A narrow strait separating the Iranian island of Qeshm from the Iranian mainland.</obo:IAO_0000115>
        <oboInOwl:hasOBONamespace>GAZ</oboInOwl:hasOBONamespace>
        <oboInOwl:id>GAZ:00250922</oboInOwl:id>
        <rdfs:label>Khouran Strait</rdfs:label>
    </owl:NamedIndividual>
    


    <!-- http://purl.obolibrary.org/obo/GAZ_00250926 -->

    <owl:NamedIndividual rdf:about="http://purl.obolibrary.org/obo/GAZ_00250926">
        <obo:IAO_0000115>A shallow bay.</obo:IAO_0000115>
        <oboInOwl:hasOBONamespace>GAZ</oboInOwl:hasOBONamespace>
        <oboInOwl:id>GAZ:00250926</oboInOwl:id>
        <rdfs:label>Khor Tiab</rdfs:label>
    </owl:NamedIndividual>
    


    <!-- http://purl.obolibrary.org/obo/GAZ_00250927 -->

    <owl:NamedIndividual rdf:about="http://purl.obolibrary.org/obo/GAZ_00250927">
        <obo:IAO_0000115>A shallow bay.</obo:IAO_0000115>
        <oboInOwl:hasOBONamespace>GAZ</oboInOwl:hasOBONamespace>
        <oboInOwl:id>GAZ:00250927</oboInOwl:id>
        <rdfs:label>Khor Kolahy</rdfs:label>
    </owl:NamedIndividual>
    


    <!-- http://purl.obolibrary.org/obo/GAZ_00251031 -->

    <owl:NamedIndividual rdf:about="http://purl.obolibrary.org/obo/GAZ_00251031">
        <obo:IAO_0000115>A canal which links the southeast corner of Haur Al Hammar to the head of the Gulf via Khawr Al Zubair.</obo:IAO_0000115>
        <oboInOwl:hasOBONamespace>GAZ</oboInOwl:hasOBONamespace>
        <oboInOwl:id>GAZ:00251031</oboInOwl:id>
        <rdfs:label>Shatt Al Basrah</rdfs:label>
    </owl:NamedIndividual>
    


    <!-- http://purl.obolibrary.org/obo/GAZ_00251076 -->

    <owl:NamedIndividual rdf:about="http://purl.obolibrary.org/obo/GAZ_00251076">
        <obo:IAO_0000115>A tidal inlet at the head of the Persian Gulf. It receives freshwater inflow from the Shatt Al Basrah ) at its northern end, and opens up into Khawr Abd Allah in the southeast.</obo:IAO_0000115>
        <oboInOwl:hasOBONamespace>GAZ</oboInOwl:hasOBONamespace>
        <oboInOwl:id>GAZ:00251076</oboInOwl:id>
        <rdfs:label>Khawr Al Zubair</rdfs:label>
    </owl:NamedIndividual>
    


    <!-- http://purl.obolibrary.org/obo/GAZ_00251769 -->

    <owl:NamedIndividual rdf:about="http://purl.obolibrary.org/obo/GAZ_00251769">
        <obo:RO_0001025 rdf:resource="http://purl.obolibrary.org/obo/GAZ_00018501"/>
        <obo:IAO_0000115>A shallow sea bay with inter-tidal mudflats. Located at the west end of Kuwait Bay, about 25 km west of Kuwait City centre, Al-Jahra Region.</obo:IAO_0000115>
        <oboInOwl:hasOBONamespace>GAZ</oboInOwl:hasOBONamespace>
        <oboInOwl:id>GAZ:00251769</oboInOwl:id>
        <rdfs:label>Dawhat Kazima</rdfs:label>
    </owl:NamedIndividual>
    


    <!-- http://purl.obolibrary.org/obo/GAZ_00251770 -->

    <owl:NamedIndividual rdf:about="http://purl.obolibrary.org/obo/GAZ_00251770">
        <obo:RO_0001025 rdf:resource="http://purl.obolibrary.org/obo/GAZ_00018501"/>
        <obo:IAO_0000115>A very shallow, sheltered bay on the south side of Kuwait Bay.</obo:IAO_0000115>
        <oboInOwl:hasOBONamespace>GAZ</oboInOwl:hasOBONamespace>
        <oboInOwl:id>GAZ:00251770</oboInOwl:id>
        <rdfs:label>Sulaibikhat Bay</rdfs:label>
    </owl:NamedIndividual>
    


    <!-- http://purl.obolibrary.org/obo/GAZ_00255670 -->

    <owl:NamedIndividual rdf:about="http://purl.obolibrary.org/obo/GAZ_00255670">
        <obo:RO_0001025 rdf:resource="http://purl.obolibrary.org/obo/GAZ_00053716"/>
        <obo:IAO_0000115>A lava cave(s).</obo:IAO_0000115>
        <oboInOwl:hasOBONamespace>GAZ</oboInOwl:hasOBONamespace>
        <oboInOwl:id>GAZ:00255670</oboInOwl:id>
        <rdfs:label>Harrat Kishb Caves</rdfs:label>
    </owl:NamedIndividual>
    


    <!-- http://purl.obolibrary.org/obo/GAZ_00255671 -->

    <owl:NamedIndividual rdf:about="http://purl.obolibrary.org/obo/GAZ_00255671">
        <obo:RO_0001025 rdf:resource="http://purl.obolibrary.org/obo/GAZ_00053716"/>
        <obo:IAO_0000115>A lava cave(s).</obo:IAO_0000115>
        <oboInOwl:hasOBONamespace>GAZ</oboInOwl:hasOBONamespace>
        <oboInOwl:id>GAZ:00255671</oboInOwl:id>
        <rdfs:label>Mut&apos;eb Cave</rdfs:label>
    </owl:NamedIndividual>
    


    <!-- http://purl.obolibrary.org/obo/GAZ_00255672 -->

    <owl:NamedIndividual rdf:about="http://purl.obolibrary.org/obo/GAZ_00255672">
        <obo:RO_0001025 rdf:resource="http://purl.obolibrary.org/obo/GAZ_00053716"/>
        <obo:IAO_0000115>A lava cave(s).</obo:IAO_0000115>
        <oboInOwl:hasOBONamespace>GAZ</oboInOwl:hasOBONamespace>
        <oboInOwl:id>GAZ:00255672</oboInOwl:id>
        <rdfs:label>Kahf Al Ashbaah</rdfs:label>
    </owl:NamedIndividual>
    


    <!-- http://purl.obolibrary.org/obo/GAZ_00255673 -->

    <owl:NamedIndividual rdf:about="http://purl.obolibrary.org/obo/GAZ_00255673">
        <obo:RO_0001025 rdf:resource="http://purl.obolibrary.org/obo/GAZ_00053716"/>
        <obo:IAO_0000115>A lava cave(s).</obo:IAO_0000115>
        <oboInOwl:hasOBONamespace>GAZ</oboInOwl:hasOBONamespace>
        <oboInOwl:id>GAZ:00255673</oboInOwl:id>
        <rdfs:label>Dahl Faisal</rdfs:label>
    </owl:NamedIndividual>
    


    <!-- http://purl.obolibrary.org/obo/GAZ_00255674 -->

    <owl:NamedIndividual rdf:about="http://purl.obolibrary.org/obo/GAZ_00255674">
        <obo:RO_0001025 rdf:resource="http://purl.obolibrary.org/obo/GAZ_00005295"/>
        <obo:RO_0001025 rdf:resource="http://purl.obolibrary.org/obo/GAZ_00015058"/>
        <obo:IAO_0000115>A bay. Located between Jubail and Abu Ali in the south-southeast and Ra&apos;s as Zawr in the northwest.</obo:IAO_0000115>
        <oboInOwl:hasOBONamespace>GAZ</oboInOwl:hasOBONamespace>
        <oboInOwl:id>GAZ:00255674</oboInOwl:id>
        <rdfs:label>Dawhat ad-Dafi</rdfs:label>
    </owl:NamedIndividual>
    


    <!-- http://purl.obolibrary.org/obo/GAZ_00255675 -->

    <owl:NamedIndividual rdf:about="http://purl.obolibrary.org/obo/GAZ_00255675">
        <obo:RO_0001025 rdf:resource="http://purl.obolibrary.org/obo/GAZ_00005295"/>
        <obo:RO_0001025 rdf:resource="http://purl.obolibrary.org/obo/GAZ_00015058"/>
        <obo:IAO_0000115>A bay. Located between Jubail and Abu Ali in the south-southeast and Ra&apos;s as Zawr in the northwest.</obo:IAO_0000115>
        <oboInOwl:hasOBONamespace>GAZ</oboInOwl:hasOBONamespace>
        <oboInOwl:id>GAZ:00255675</oboInOwl:id>
        <rdfs:label>Dawhat al-Musallamiya</rdfs:label>
    </owl:NamedIndividual>
    


    <!-- http://purl.obolibrary.org/obo/GAZ_00255676 -->

    <owl:NamedIndividual rdf:about="http://purl.obolibrary.org/obo/GAZ_00255676">
        <obo:RO_0001025 rdf:resource="http://purl.obolibrary.org/obo/GAZ_00005295"/>
        <obo:RO_0001025 rdf:resource="http://purl.obolibrary.org/obo/GAZ_00015058"/>
        <obo:IAO_0000115>An island. Located close to shore northeast of Jubail. Connected to the mainland north of Jubail Industrial City by causeway.</obo:IAO_0000115>
        <oboInOwl:hasOBONamespace>GAZ</oboInOwl:hasOBONamespace>
        <oboInOwl:id>GAZ:00255676</oboInOwl:id>
        <rdfs:label>Batima</rdfs:label>
    </owl:NamedIndividual>
    


    <!-- http://purl.obolibrary.org/obo/GAZ_00255677 -->

    <owl:NamedIndividual rdf:about="http://purl.obolibrary.org/obo/GAZ_00255677">
        <obo:RO_0001025 rdf:resource="http://purl.obolibrary.org/obo/GAZ_00005295"/>
        <obo:RO_0001025 rdf:resource="http://purl.obolibrary.org/obo/GAZ_00015058"/>
        <obo:IAO_0000115>An island. Located close to shore northeast of Jubail. Connected to the mainland north of Jubail Industrial City by causeway.</obo:IAO_0000115>
        <oboInOwl:hasOBONamespace>GAZ</oboInOwl:hasOBONamespace>
        <oboInOwl:id>GAZ:00255677</oboInOwl:id>
        <rdfs:label>Abu Ali</rdfs:label>
    </owl:NamedIndividual>
    


    <!-- http://purl.obolibrary.org/obo/GAZ_00255678 -->

    <owl:NamedIndividual rdf:about="http://purl.obolibrary.org/obo/GAZ_00255678">
        <obo:RO_0001025 rdf:resource="http://purl.obolibrary.org/obo/GAZ_00015058"/>
        <obo:IAO_0000115>Man-made evaporation lagoons. Located on the southwest edge of Jubail Industrial City, Eastern Province.</obo:IAO_0000115>
        <oboInOwl:hasOBONamespace>GAZ</oboInOwl:hasOBONamespace>
        <oboInOwl:id>GAZ:00255678</oboInOwl:id>
        <rdfs:label>Sabkhat al-Fasl Lagoons</rdfs:label>
    </owl:NamedIndividual>
    


    <!-- http://purl.obolibrary.org/obo/GAZ_00255679 -->

    <owl:NamedIndividual rdf:about="http://purl.obolibrary.org/obo/GAZ_00255679">
        <obo:RO_0001025 rdf:resource="http://purl.obolibrary.org/obo/GAZ_00005295"/>
        <obo:RO_0001025 rdf:resource="http://purl.obolibrary.org/obo/GAZ_00015058"/>
        <obo:IAO_0000115>A group of coral islands situated about 35-90 km offshore.</obo:IAO_0000115>
        <oboInOwl:hasOBONamespace>GAZ</oboInOwl:hasOBONamespace>
        <oboInOwl:id>GAZ:00255679</oboInOwl:id>
        <rdfs:label>Gulf Coral Islands</rdfs:label>
    </owl:NamedIndividual>
    


    <!-- http://purl.obolibrary.org/obo/GAZ_00255680 -->

    <owl:NamedIndividual rdf:about="http://purl.obolibrary.org/obo/GAZ_00255680">
        <obo:RO_0001025 rdf:resource="http://purl.obolibrary.org/obo/GAZ_00255679"/>
        <obo:IAO_0000115>A coral island.</obo:IAO_0000115>
        <oboInOwl:hasOBONamespace>GAZ</oboInOwl:hasOBONamespace>
        <oboInOwl:id>GAZ:00255680</oboInOwl:id>
        <rdfs:label>Jazirat al Jurayd</rdfs:label>
    </owl:NamedIndividual>
    


    <!-- http://purl.obolibrary.org/obo/GAZ_00255681 -->

    <owl:NamedIndividual rdf:about="http://purl.obolibrary.org/obo/GAZ_00255681">
        <obo:RO_0001025 rdf:resource="http://purl.obolibrary.org/obo/GAZ_00255679"/>
        <obo:IAO_0000115>A coral island.</obo:IAO_0000115>
        <oboInOwl:hasOBONamespace>GAZ</oboInOwl:hasOBONamespace>
        <oboInOwl:id>GAZ:00255681</oboInOwl:id>
        <rdfs:label>Jazirat Karan</rdfs:label>
    </owl:NamedIndividual>
    


    <!-- http://purl.obolibrary.org/obo/GAZ_00255682 -->

    <owl:NamedIndividual rdf:about="http://purl.obolibrary.org/obo/GAZ_00255682">
        <obo:RO_0001025 rdf:resource="http://purl.obolibrary.org/obo/GAZ_00255679"/>
        <obo:IAO_0000115>A coral island.</obo:IAO_0000115>
        <oboInOwl:hasOBONamespace>GAZ</oboInOwl:hasOBONamespace>
        <oboInOwl:id>GAZ:00255682</oboInOwl:id>
        <rdfs:label>Jazirat Kurayn</rdfs:label>
    </owl:NamedIndividual>
    


    <!-- http://purl.obolibrary.org/obo/GAZ_00255683 -->

    <owl:NamedIndividual rdf:about="http://purl.obolibrary.org/obo/GAZ_00255683">
        <obo:RO_0001025 rdf:resource="http://purl.obolibrary.org/obo/GAZ_00255679"/>
        <obo:IAO_0000115>A coral island.</obo:IAO_0000115>
        <oboInOwl:hasOBONamespace>GAZ</oboInOwl:hasOBONamespace>
        <oboInOwl:id>GAZ:00255683</oboInOwl:id>
        <rdfs:label>Jazirat Jana</rdfs:label>
    </owl:NamedIndividual>
    


    <!-- http://purl.obolibrary.org/obo/GAZ_00255684 -->

    <owl:NamedIndividual rdf:about="http://purl.obolibrary.org/obo/GAZ_00255684">
        <obo:RO_0001025 rdf:resource="http://purl.obolibrary.org/obo/GAZ_00255679"/>
        <obo:IAO_0000115>A coral island.</obo:IAO_0000115>
        <oboInOwl:hasOBONamespace>GAZ</oboInOwl:hasOBONamespace>
        <oboInOwl:id>GAZ:00255684</oboInOwl:id>
        <rdfs:label>Jazirat Harqus</rdfs:label>
    </owl:NamedIndividual>
    


    <!-- http://purl.obolibrary.org/obo/GAZ_00255685 -->

    <owl:NamedIndividual rdf:about="http://purl.obolibrary.org/obo/GAZ_00255685">
        <obo:RO_0001025 rdf:resource="http://purl.obolibrary.org/obo/GAZ_00255679"/>
        <obo:IAO_0000115>A coral island.</obo:IAO_0000115>
        <oboInOwl:hasOBONamespace>GAZ</oboInOwl:hasOBONamespace>
        <oboInOwl:id>GAZ:00255685</oboInOwl:id>
        <rdfs:label>Jazirat al-Arabiyah</rdfs:label>
    </owl:NamedIndividual>
    


    <!-- http://purl.obolibrary.org/obo/GAZ_00255686 -->

    <owl:NamedIndividual rdf:about="http://purl.obolibrary.org/obo/GAZ_00255686">
        <obo:RO_0001025 rdf:resource="http://purl.obolibrary.org/obo/GAZ_00005295"/>
        <obo:RO_0001025 rdf:resource="http://purl.obolibrary.org/obo/GAZ_00015058"/>
        <obo:IAO_0000115>A bay. Located on the Gulf coast east of Qatif and north of Dammam, Eastern Province.</obo:IAO_0000115>
        <oboInOwl:hasOBONamespace>GAZ</oboInOwl:hasOBONamespace>
        <oboInOwl:id>GAZ:00255686</oboInOwl:id>
        <rdfs:label>Tarut Bay</rdfs:label>
    </owl:NamedIndividual>
    


    <!-- http://purl.obolibrary.org/obo/GAZ_00255687 -->

    <owl:NamedIndividual rdf:about="http://purl.obolibrary.org/obo/GAZ_00255687">
        <obo:RO_0001025 rdf:resource="http://purl.obolibrary.org/obo/GAZ_00255686"/>
        <obo:IAO_0000115>An island.</obo:IAO_0000115>
        <oboInOwl:hasOBONamespace>GAZ</oboInOwl:hasOBONamespace>
        <oboInOwl:id>GAZ:00255687</oboInOwl:id>
        <rdfs:label>Za&apos;l Island</rdfs:label>
    </owl:NamedIndividual>
    


    <!-- http://purl.obolibrary.org/obo/GAZ_00255688 -->

    <owl:NamedIndividual rdf:about="http://purl.obolibrary.org/obo/GAZ_00255688">
        <obo:RO_0001025 rdf:resource="http://purl.obolibrary.org/obo/GAZ_00255686"/>
        <obo:IAO_0000115>An island. Connected to the mainland by a bridge.</obo:IAO_0000115>
        <oboInOwl:hasOBONamespace>GAZ</oboInOwl:hasOBONamespace>
        <oboInOwl:id>GAZ:00255688</oboInOwl:id>
        <rdfs:label>Tarut Island</rdfs:label>
    </owl:NamedIndividual>
    


    <!-- http://purl.obolibrary.org/obo/GAZ_00255689 -->

    <owl:NamedIndividual rdf:about="http://purl.obolibrary.org/obo/GAZ_00255689">
        <obo:RO_0001025 rdf:resource="http://purl.obolibrary.org/obo/GAZ_00015058"/>
        <obo:IAO_0000115>A wetland. Freshwater lagoons. Formed primarily from run-off from al-Hasa oasis. The wetland comprises a long, narrow river, flowing in an eastsoutheast direction from Hofuf and Abqaiq towards al-&apos;Uqair. Often, the river goes underground beneath sand dunes for several kilometres before resurfacing. There are many pools, some of which can be quite large, up to 250 ha. Located near the towns of Hofuf and Abqaiq in Eastern Province.</obo:IAO_0000115>
        <oboInOwl:hasOBONamespace>GAZ</oboInOwl:hasOBONamespace>
        <oboInOwl:id>GAZ:00255689</oboInOwl:id>
        <rdfs:label>Al-Hasa Lagoons</rdfs:label>
    </owl:NamedIndividual>
    


    <!-- http://purl.obolibrary.org/obo/GAZ_00255690 -->

    <owl:NamedIndividual rdf:about="http://purl.obolibrary.org/obo/GAZ_00255690">
        <obo:RO_0001025 rdf:resource="http://purl.obolibrary.org/obo/GAZ_00005295"/>
        <obo:IAO_0000115>The gulf between the Qatar Peninsula and the mainland of Saudi Arabia.</obo:IAO_0000115>
        <oboInOwl:hasOBONamespace>GAZ</oboInOwl:hasOBONamespace>
        <oboInOwl:id>GAZ:00255690</oboInOwl:id>
        <rdfs:label>Gulf of Salwah</rdfs:label>
    </owl:NamedIndividual>
    


    <!-- http://purl.obolibrary.org/obo/GAZ_00255691 -->

    <owl:NamedIndividual rdf:about="http://purl.obolibrary.org/obo/GAZ_00255691">
        <obo:RO_0001025 rdf:resource="http://purl.obolibrary.org/obo/GAZ_00015058"/>
        <obo:RO_0001025 rdf:resource="http://purl.obolibrary.org/obo/GAZ_00255690"/>
        <obo:IAO_0000115>An island.</obo:IAO_0000115>
        <oboInOwl:hasOBONamespace>GAZ</oboInOwl:hasOBONamespace>
        <oboInOwl:id>GAZ:00255691</oboInOwl:id>
        <rdfs:label>Jazirat az Zakhnuniyah</rdfs:label>
    </owl:NamedIndividual>
    


    <!-- http://purl.obolibrary.org/obo/GAZ_00255692 -->

    <owl:NamedIndividual rdf:about="http://purl.obolibrary.org/obo/GAZ_00255692">
        <obo:RO_0001025 rdf:resource="http://purl.obolibrary.org/obo/GAZ_00015058"/>
        <obo:RO_0001025 rdf:resource="http://purl.obolibrary.org/obo/GAZ_00255690"/>
        <obo:IAO_0000115>An island.</obo:IAO_0000115>
        <oboInOwl:hasOBONamespace>GAZ</oboInOwl:hasOBONamespace>
        <oboInOwl:id>GAZ:00255692</oboInOwl:id>
        <rdfs:label>Judhaim Island</rdfs:label>
    </owl:NamedIndividual>
    


    <!-- http://purl.obolibrary.org/obo/GAZ_00255693 -->

    <owl:NamedIndividual rdf:about="http://purl.obolibrary.org/obo/GAZ_00255693">
        <obo:RO_0001025 rdf:resource="http://purl.obolibrary.org/obo/GAZ_00015058"/>
        <obo:RO_0001025 rdf:resource="http://purl.obolibrary.org/obo/GAZ_00255690"/>
        <obo:IAO_0000115>An island.</obo:IAO_0000115>
        <oboInOwl:hasOBONamespace>GAZ</oboInOwl:hasOBONamespace>
        <oboInOwl:id>GAZ:00255693</oboInOwl:id>
        <rdfs:label>Samamik Island</rdfs:label>
    </owl:NamedIndividual>
    


    <!-- http://purl.obolibrary.org/obo/GAZ_00255694 -->

    <owl:NamedIndividual rdf:about="http://purl.obolibrary.org/obo/GAZ_00255694">
        <obo:RO_0001025 rdf:resource="http://purl.obolibrary.org/obo/GAZ_00015058"/>
        <obo:RO_0001025 rdf:resource="http://purl.obolibrary.org/obo/GAZ_00255690"/>
        <obo:IAO_0000115>An island.</obo:IAO_0000115>
        <oboInOwl:hasOBONamespace>GAZ</oboInOwl:hasOBONamespace>
        <oboInOwl:id>GAZ:00255694</oboInOwl:id>
        <rdfs:label>Unaibir Island</rdfs:label>
    </owl:NamedIndividual>
    


    <!-- http://purl.obolibrary.org/obo/GAZ_00256448 -->

    <owl:NamedIndividual rdf:about="http://purl.obolibrary.org/obo/GAZ_00256448">
        <obo:RO_0001025 rdf:resource="http://purl.obolibrary.org/obo/GAZ_00002456"/>
        <obo:IAO_0000115>A bay.</obo:IAO_0000115>
        <oboInOwl:hasOBONamespace>GAZ</oboInOwl:hasOBONamespace>
        <oboInOwl:id>GAZ:00256448</oboInOwl:id>
        <rdfs:label>Dungunab Bay</rdfs:label>
    </owl:NamedIndividual>
    


    <!-- http://purl.obolibrary.org/obo/GAZ_00256449 -->

    <owl:NamedIndividual rdf:about="http://purl.obolibrary.org/obo/GAZ_00256449">
        <obo:RO_0001025 rdf:resource="http://purl.obolibrary.org/obo/GAZ_00002456"/>
        <obo:IAO_0000115>An island.</obo:IAO_0000115>
        <oboInOwl:hasOBONamespace>GAZ</oboInOwl:hasOBONamespace>
        <oboInOwl:id>GAZ:00256449</oboInOwl:id>
        <rdfs:label>Jazirat Mukawwa&apos;</rdfs:label>
    </owl:NamedIndividual>
    


    <!-- http://purl.obolibrary.org/obo/GAZ_00260861 -->

    <owl:NamedIndividual rdf:about="http://purl.obolibrary.org/obo/GAZ_00260861">
        <obo:RO_0001025 rdf:resource="http://purl.obolibrary.org/obo/GAZ_00002456"/>
        <obo:IAO_0000115>An island.</obo:IAO_0000115>
        <oboInOwl:hasOBONamespace>GAZ</oboInOwl:hasOBONamespace>
        <oboInOwl:id>GAZ:00260861</oboInOwl:id>
        <rdfs:label>Buhays Island</rdfs:label>
    </owl:NamedIndividual>
    


    <!-- http://purl.obolibrary.org/obo/GAZ_00260862 -->

    <owl:NamedIndividual rdf:about="http://purl.obolibrary.org/obo/GAZ_00260862">
        <obo:RO_0001025 rdf:resource="http://purl.obolibrary.org/obo/GAZ_00002456"/>
        <oboInOwl:hasOBONamespace>GAZ</oboInOwl:hasOBONamespace>
        <oboInOwl:id>GAZ:00260862</oboInOwl:id>
        <rdfs:label>Al-Badi Island</rdfs:label>
    </owl:NamedIndividual>
    


    <!-- http://purl.obolibrary.org/obo/GAZ_00260863 -->

    <owl:NamedIndividual rdf:about="http://purl.obolibrary.org/obo/GAZ_00260863">
        <obo:RO_0001025 rdf:resource="http://purl.obolibrary.org/obo/GAZ_00002456"/>
        <obo:IAO_0000115>An island.</obo:IAO_0000115>
        <oboInOwl:hasOBONamespace>GAZ</oboInOwl:hasOBONamespace>
        <oboInOwl:id>GAZ:00260863</oboInOwl:id>
        <rdfs:label>Tikfash Island</rdfs:label>
    </owl:NamedIndividual>
    


    <!-- http://purl.obolibrary.org/obo/GAZ_00260864 -->

    <owl:NamedIndividual rdf:about="http://purl.obolibrary.org/obo/GAZ_00260864">
        <obo:RO_0001025 rdf:resource="http://purl.obolibrary.org/obo/GAZ_00002456"/>
        <obo:IAO_0000115>An island.</obo:IAO_0000115>
        <oboInOwl:hasOBONamespace>GAZ</oboInOwl:hasOBONamespace>
        <oboInOwl:id>GAZ:00260864</oboInOwl:id>
        <rdfs:label>Humar Island</rdfs:label>
    </owl:NamedIndividual>
    


    <!-- http://purl.obolibrary.org/obo/GAZ_00260865 -->

    <owl:NamedIndividual rdf:about="http://purl.obolibrary.org/obo/GAZ_00260865">
        <obo:RO_0001025 rdf:resource="http://purl.obolibrary.org/obo/GAZ_00002456"/>
        <obo:IAO_0000115>An island.</obo:IAO_0000115>
        <oboInOwl:hasOBONamespace>GAZ</oboInOwl:hasOBONamespace>
        <oboInOwl:id>GAZ:00260865</oboInOwl:id>
        <rdfs:label>Kitamah Island</rdfs:label>
    </owl:NamedIndividual>
    


    <!-- http://purl.obolibrary.org/obo/GAZ_00260866 -->

    <owl:NamedIndividual rdf:about="http://purl.obolibrary.org/obo/GAZ_00260866">
        <obo:RO_0001025 rdf:resource="http://purl.obolibrary.org/obo/GAZ_00002456"/>
        <obo:IAO_0000115>An island.</obo:IAO_0000115>
        <oboInOwl:hasOBONamespace>GAZ</oboInOwl:hasOBONamespace>
        <oboInOwl:id>GAZ:00260866</oboInOwl:id>
        <rdfs:label>Zakhah Island</rdfs:label>
    </owl:NamedIndividual>
    


    <!-- http://purl.obolibrary.org/obo/GAZ_00260867 -->

    <owl:NamedIndividual rdf:about="http://purl.obolibrary.org/obo/GAZ_00260867">
        <obo:RO_0001025 rdf:resource="http://purl.obolibrary.org/obo/GAZ_00002456"/>
        <obo:IAO_0000115>An island.</obo:IAO_0000115>
        <oboInOwl:hasOBONamespace>GAZ</oboInOwl:hasOBONamespace>
        <oboInOwl:id>GAZ:00260867</oboInOwl:id>
        <rdfs:label>Zurbat Island</rdfs:label>
    </owl:NamedIndividual>
    


    <!-- http://purl.obolibrary.org/obo/GAZ_00260868 -->

    <owl:NamedIndividual rdf:about="http://purl.obolibrary.org/obo/GAZ_00260868">
        <obo:RO_0001025 rdf:resource="http://purl.obolibrary.org/obo/GAZ_00002456"/>
        <obo:IAO_0000115>An island.</obo:IAO_0000115>
        <oboInOwl:hasOBONamespace>GAZ</oboInOwl:hasOBONamespace>
        <oboInOwl:id>GAZ:00260868</oboInOwl:id>
        <rdfs:label>Juwa Island</rdfs:label>
    </owl:NamedIndividual>
    


    <!-- http://purl.obolibrary.org/obo/GAZ_00260869 -->

    <owl:NamedIndividual rdf:about="http://purl.obolibrary.org/obo/GAZ_00260869">
        <obo:RO_0001025 rdf:resource="http://purl.obolibrary.org/obo/GAZ_00002456"/>
        <obo:IAO_0000115>An island.</obo:IAO_0000115>
        <oboInOwl:hasOBONamespace>GAZ</oboInOwl:hasOBONamespace>
        <oboInOwl:id>GAZ:00260869</oboInOwl:id>
        <rdfs:label>At Talawin Island</rdfs:label>
    </owl:NamedIndividual>
    


    <!-- http://purl.obolibrary.org/obo/GAZ_00260871 -->

    <owl:NamedIndividual rdf:about="http://purl.obolibrary.org/obo/GAZ_00260871">
        <obo:RO_0001025 rdf:resource="http://purl.obolibrary.org/obo/GAZ_00002456"/>
        <obo:IAO_0000115>An island.</obo:IAO_0000115>
        <oboInOwl:hasOBONamespace>GAZ</oboInOwl:hasOBONamespace>
        <oboInOwl:id>GAZ:00260871</oboInOwl:id>
        <rdfs:label>Zabin Island</rdfs:label>
    </owl:NamedIndividual>
    


    <!-- http://purl.obolibrary.org/obo/GAZ_00260872 -->

    <owl:NamedIndividual rdf:about="http://purl.obolibrary.org/obo/GAZ_00260872">
        <obo:RO_0001025 rdf:resource="http://purl.obolibrary.org/obo/GAZ_00002456"/>
        <obo:IAO_0000115>An island.</obo:IAO_0000115>
        <oboInOwl:hasOBONamespace>GAZ</oboInOwl:hasOBONamespace>
        <oboInOwl:id>GAZ:00260872</oboInOwl:id>
        <rdfs:label>Al-Murk Island</rdfs:label>
    </owl:NamedIndividual>
    


    <!-- http://purl.obolibrary.org/obo/GAZ_00260873 -->

    <owl:NamedIndividual rdf:about="http://purl.obolibrary.org/obo/GAZ_00260873">
        <obo:RO_0001025 rdf:resource="http://purl.obolibrary.org/obo/GAZ_00002456"/>
        <obo:IAO_0000115>An island.</obo:IAO_0000115>
        <oboInOwl:hasOBONamespace>GAZ</oboInOwl:hasOBONamespace>
        <oboInOwl:id>GAZ:00260873</oboInOwl:id>
        <rdfs:label>Hataban Island</rdfs:label>
    </owl:NamedIndividual>
    


    <!-- http://purl.obolibrary.org/obo/GAZ_00260874 -->

    <owl:NamedIndividual rdf:about="http://purl.obolibrary.org/obo/GAZ_00260874">
        <obo:RO_0001025 rdf:resource="http://purl.obolibrary.org/obo/GAZ_00002456"/>
        <obo:IAO_0000115>An island.</obo:IAO_0000115>
        <oboInOwl:hasOBONamespace>GAZ</oboInOwl:hasOBONamespace>
        <oboInOwl:id>GAZ:00260874</oboInOwl:id>
        <rdfs:label>&apos;Ukban Island</rdfs:label>
    </owl:NamedIndividual>
    


    <!-- http://purl.obolibrary.org/obo/GAZ_00260875 -->

    <owl:NamedIndividual rdf:about="http://purl.obolibrary.org/obo/GAZ_00260875">
        <obo:RO_0001025 rdf:resource="http://purl.obolibrary.org/obo/GAZ_00002456"/>
        <obo:IAO_0000115>An island.</obo:IAO_0000115>
        <oboInOwl:hasOBONamespace>GAZ</oboInOwl:hasOBONamespace>
        <oboInOwl:id>GAZ:00260875</oboInOwl:id>
        <rdfs:label>Bahr Ibn Abbas</rdfs:label>
    </owl:NamedIndividual>
    


    <!-- http://purl.obolibrary.org/obo/GAZ_02000358 -->

    <owl:NamedIndividual rdf:about="http://purl.obolibrary.org/obo/GAZ_02000358"/>
    


    <!-- http://purl.obolibrary.org/obo/GAZ_02000359 -->

    <owl:NamedIndividual rdf:about="http://purl.obolibrary.org/obo/GAZ_02000359">
        <obo:RO_0001025 rdf:resource="http://purl.obolibrary.org/obo/GAZ_00006938"/>
    </owl:NamedIndividual>
    


    <!-- http://purl.obolibrary.org/obo/GAZ_02000360 -->

    <owl:NamedIndividual rdf:about="http://purl.obolibrary.org/obo/GAZ_02000360"/>
    


    <!-- http://purl.obolibrary.org/obo/GAZ_02000361 -->

    <owl:NamedIndividual rdf:about="http://purl.obolibrary.org/obo/GAZ_02000361"/>
    


    <!-- http://purl.obolibrary.org/obo/GAZ_02000362 -->

    <owl:NamedIndividual rdf:about="http://purl.obolibrary.org/obo/GAZ_02000362"/>
    


    <!-- http://purl.obolibrary.org/obo/GAZ_22225212 -->

    <owl:NamedIndividual rdf:about="http://purl.obolibrary.org/obo/GAZ_22225212">
        <obo:RO_0001025 rdf:resource="http://purl.obolibrary.org/obo/GAZ_00031295"/>
        <oboInOwl:hasOBONamespace>GAZ</oboInOwl:hasOBONamespace>
        <oboInOwl:id>GAZ:22225212</oboInOwl:id>
        <rdfs:label>Jeddah</rdfs:label>
    </owl:NamedIndividual>
    


    <!-- http://purl.obolibrary.org/obo/GAZ_22225213 -->

    <owl:NamedIndividual rdf:about="http://purl.obolibrary.org/obo/GAZ_22225213">
        <obo:RO_0001025 rdf:resource="http://purl.obolibrary.org/obo/GAZ_00031319"/>
        <oboInOwl:hasOBONamespace>GAZ</oboInOwl:hasOBONamespace>
        <oboInOwl:id>GAZ:22225213</oboInOwl:id>
        <rdfs:label>Najran</rdfs:label>
    </owl:NamedIndividual>
    


    <!-- 
    ///////////////////////////////////////////////////////////////////////////////////////
    //
    // Annotations
    //
    ///////////////////////////////////////////////////////////////////////////////////////
     -->

    <rdf:Description rdf:about="http://purl.obolibrary.org/obo/GAZ_00007506">
        <oboInOwl:id>GAZ:00007506</oboInOwl:id>
        <obo:IAO_0000115>The most populous province of Saudi Arabia, located in the west of the country, with an extended coastline. Its capital is the sacred city of Mecca, but its largest city is Jeddah, which is also Saudi Arabia&apos;s main port city.</obo:IAO_0000115>
        <oboInOwl:hasOBONamespace>GAZ</oboInOwl:hasOBONamespace>
        <rdfs:label>Makkah Province</rdfs:label>
    </rdf:Description>
    <rdf:Description rdf:about="http://purl.obolibrary.org/obo/GAZ_00007507">
        <oboInOwl:hasOBONamespace>GAZ</oboInOwl:hasOBONamespace>
        <oboInOwl:id>GAZ:00007507</oboInOwl:id>
        <rdfs:label>Mecca</rdfs:label>
    </rdf:Description>
    <rdf:Description rdf:about="http://purl.obolibrary.org/obo/GAZ_00007508">
        <oboInOwl:hasOBONamespace>GAZ</oboInOwl:hasOBONamespace>
        <oboInOwl:id>GAZ:00007508</oboInOwl:id>
        <rdfs:label>populated place, Saudi Arabia</rdfs:label>
    </rdf:Description>
    <rdf:Description rdf:about="http://purl.obolibrary.org/obo/GAZ_00007509">
        <oboInOwl:hasOBONamespace>GAZ</oboInOwl:hasOBONamespace>
        <oboInOwl:id>GAZ:00007509</oboInOwl:id>
        <rdfs:label>Province (Saudi Arabia)</rdfs:label>
    </rdf:Description>
    <rdf:Description rdf:about="http://purl.obolibrary.org/obo/GAZ_00009519">
        <oboInOwl:id>GAZ:00009519</oboInOwl:id>
        <rdfs:label>Governorate (Bahrain)</rdfs:label>
        <oboInOwl:hasOBONamespace>GAZ</oboInOwl:hasOBONamespace>
    </rdf:Description>
    <rdf:Description rdf:about="http://purl.obolibrary.org/obo/GAZ_00010395">
        <oboInOwl:hasOBONamespace>GAZ</oboInOwl:hasOBONamespace>
        <rdfs:label>Ar Riyadh Province</rdfs:label>
        <oboInOwl:id>GAZ:00010395</oboInOwl:id>
    </rdf:Description>
    <rdf:Description rdf:about="http://purl.obolibrary.org/obo/GAZ_00010396">
        <rdfs:label>Riyadh</rdfs:label>
        <oboInOwl:id>GAZ:00010396</oboInOwl:id>
        <oboInOwl:hasOBONamespace>GAZ</oboInOwl:hasOBONamespace>
    </rdf:Description>
    <rdf:Description rdf:about="http://purl.obolibrary.org/obo/GAZ_00010397">
        <oboInOwl:id>GAZ:00010397</oboInOwl:id>
        <oboInOwl:hasOBONamespace>GAZ</oboInOwl:hasOBONamespace>
        <rdfs:label>Asir Province</rdfs:label>
    </rdf:Description>
    <rdf:Description rdf:about="http://purl.obolibrary.org/obo/GAZ_00010398">
        <rdfs:label>Jizan Province</rdfs:label>
        <oboInOwl:id>GAZ:00010398</oboInOwl:id>
        <oboInOwl:hasOBONamespace>GAZ</oboInOwl:hasOBONamespace>
    </rdf:Description>
    <rdf:Description rdf:about="http://purl.obolibrary.org/obo/GAZ_00015054">
        <rdfs:label>Tabuk Province</rdfs:label>
        <oboInOwl:id>GAZ:00015054</oboInOwl:id>
        <oboInOwl:hasOBONamespace>GAZ</oboInOwl:hasOBONamespace>
    </rdf:Description>
    <rdf:Description rdf:about="http://purl.obolibrary.org/obo/GAZ_00015055">
        <oboInOwl:id>GAZ:00015055</oboInOwl:id>
        <rdfs:label>Al Qasim Province</rdfs:label>
        <oboInOwl:hasOBONamespace>GAZ</oboInOwl:hasOBONamespace>
    </rdf:Description>
    <rdf:Description rdf:about="http://purl.obolibrary.org/obo/GAZ_00015056">
        <oboInOwl:id>GAZ:00015056</oboInOwl:id>
        <rdfs:label>Najran Province</rdfs:label>
        <oboInOwl:hasOBONamespace>GAZ</oboInOwl:hasOBONamespace>
    </rdf:Description>
    <rdf:Description rdf:about="http://purl.obolibrary.org/obo/GAZ_00015057">
        <oboInOwl:id>GAZ:00015057</oboInOwl:id>
        <rdfs:label>Northan Border Province</rdfs:label>
        <oboInOwl:hasOBONamespace>GAZ</oboInOwl:hasOBONamespace>
    </rdf:Description>
    <rdf:Description rdf:about="http://purl.obolibrary.org/obo/GAZ_00015058">
        <oboInOwl:id>GAZ:00015058</oboInOwl:id>
        <rdfs:label>Eastern Province</rdfs:label>
        <oboInOwl:hasOBONamespace>GAZ</oboInOwl:hasOBONamespace>
    </rdf:Description>
    <rdf:Description rdf:about="http://purl.obolibrary.org/obo/GAZ_00015059">
        <oboInOwl:id>GAZ:00015059</oboInOwl:id>
        <rdfs:label>Al Jawf Province</rdfs:label>
        <oboInOwl:hasOBONamespace>GAZ</oboInOwl:hasOBONamespace>
    </rdf:Description>
    <rdf:Description rdf:about="http://purl.obolibrary.org/obo/GAZ_00015060">
        <rdfs:label>Medina Province</rdfs:label>
        <oboInOwl:id>GAZ:00015060</oboInOwl:id>
        <oboInOwl:hasOBONamespace>GAZ</oboInOwl:hasOBONamespace>
    </rdf:Description>
    <rdf:Description rdf:about="http://purl.obolibrary.org/obo/GAZ_00015061">
        <rdfs:label>Ha&apos;il Province</rdfs:label>
        <oboInOwl:id>GAZ:00015061</oboInOwl:id>
        <oboInOwl:hasOBONamespace>GAZ</oboInOwl:hasOBONamespace>
    </rdf:Description>
    <rdf:Description rdf:about="http://purl.obolibrary.org/obo/GAZ_00015062">
        <rdfs:label>Al Bahah Province</rdfs:label>
        <oboInOwl:id>GAZ:00015062</oboInOwl:id>
        <oboInOwl:hasOBONamespace>GAZ</oboInOwl:hasOBONamespace>
    </rdf:Description>
    <rdf:Description rdf:about="http://purl.obolibrary.org/obo/GAZ_02000358">
        <oboInOwl:id>GAZ:02000358</oboInOwl:id>
        <obo:IAO_0000115>The largest of the five governorates of Bahrain.</obo:IAO_0000115>
        <oboInOwl:hasOBONamespace>GAZ</oboInOwl:hasOBONamespace>
        <rdfs:label>Southern Governorate</rdfs:label>
    </rdf:Description>
    <rdf:Description rdf:about="http://purl.obolibrary.org/obo/GAZ_02000359">
        <oboInOwl:id>GAZ:02000359</oboInOwl:id>
        <rdfs:label>Al Muharraq Governorate</rdfs:label>
        <obo:IAO_0000115>One of the five governorates of Bahrain.</obo:IAO_0000115>
        <oboInOwl:hasOBONamespace>GAZ</oboInOwl:hasOBONamespace>
    </rdf:Description>
    <rdf:Description rdf:about="http://purl.obolibrary.org/obo/GAZ_02000360">
        <rdfs:label>Northern Governorate</rdfs:label>
        <oboInOwl:hasOBONamespace>GAZ</oboInOwl:hasOBONamespace>
        <obo:IAO_0000115>One of the five governorates of Bahrain.</obo:IAO_0000115>
        <oboInOwl:id>GAZ:02000360</oboInOwl:id>
    </rdf:Description>
    <rdf:Description rdf:about="http://purl.obolibrary.org/obo/GAZ_02000361">
        <rdfs:label>Central Governorate</rdfs:label>
        <oboInOwl:hasOBONamespace>GAZ</oboInOwl:hasOBONamespace>
        <oboInOwl:id>GAZ:02000361</oboInOwl:id>
        <obo:IAO_0000115>One of the five governorates of Bahrain.</obo:IAO_0000115>
    </rdf:Description>
    <rdf:Description rdf:about="http://purl.obolibrary.org/obo/GAZ_02000362">
        <rdfs:label>Capital Governorate</rdfs:label>
        <oboInOwl:hasOBONamespace>GAZ</oboInOwl:hasOBONamespace>
        <obo:IAO_0000115>One of the five governorates of Bahrain.</obo:IAO_0000115>
        <oboInOwl:id>GAZ:02000362</oboInOwl:id>
    </rdf:Description>
</rdf:RDF>



<!-- Generated by the OWL API (version 4.5.6) https://github.com/owlcs/owlapi -->

