<?xml version="1.0"?>
<rdf:RDF xmlns="http://purl.obolibrary.org/obo/gaz/subsets/countries/Solomon_Islands.owl#"
     xml:base="http://purl.obolibrary.org/obo/gaz/subsets/countries/Solomon_Islands.owl"
     xmlns:obo="http://purl.obolibrary.org/obo/"
     xmlns:owl="http://www.w3.org/2002/07/owl#"
     xmlns:rdf="http://www.w3.org/1999/02/22-rdf-syntax-ns#"
     xmlns:xml="http://www.w3.org/XML/1998/namespace"
     xmlns:xsd="http://www.w3.org/2001/XMLSchema#"
     xmlns:rdfs="http://www.w3.org/2000/01/rdf-schema#"
     xmlns:oboInOwl="http://www.geneontology.org/formats/oboInOwl#">
    <owl:Ontology rdf:about="http://purl.obolibrary.org/obo/gaz/subsets/countries/Solomon_Islands.owl">
        <owl:imports rdf:resource="http://purl.obolibrary.org/obo/gaz/imports/envo_import.owl"/>
        <owl:imports rdf:resource="http://purl.obolibrary.org/obo/gaz/imports/ro_import.owl"/>
    </owl:Ontology>
    


    <!-- 
    ///////////////////////////////////////////////////////////////////////////////////////
    //
    // Annotation properties
    //
    ///////////////////////////////////////////////////////////////////////////////////////
     -->

    


    <!-- http://purl.obolibrary.org/obo/IAO_0000115 -->

    <owl:AnnotationProperty rdf:about="http://purl.obolibrary.org/obo/IAO_0000115"/>
    


    <!-- http://www.geneontology.org/formats/oboInOwl#hasOBONamespace -->

    <owl:AnnotationProperty rdf:about="http://www.geneontology.org/formats/oboInOwl#hasOBONamespace"/>
    


    <!-- http://www.geneontology.org/formats/oboInOwl#id -->

    <owl:AnnotationProperty rdf:about="http://www.geneontology.org/formats/oboInOwl#id"/>
    


    <!-- 
    ///////////////////////////////////////////////////////////////////////////////////////
    //
    // Object Properties
    //
    ///////////////////////////////////////////////////////////////////////////////////////
     -->

    


    <!-- http://purl.obolibrary.org/obo/RO_0001025 -->

    <owl:ObjectProperty rdf:about="http://purl.obolibrary.org/obo/RO_0001025"/>
    


    <!-- 
    ///////////////////////////////////////////////////////////////////////////////////////
    //
    // Classes
    //
    ///////////////////////////////////////////////////////////////////////////////////////
     -->

    


    <!-- http://purl.obolibrary.org/obo/ENVO_00000029 -->

    <owl:Class rdf:about="http://purl.obolibrary.org/obo/ENVO_00000029"/>
    


    <!-- http://purl.obolibrary.org/obo/ENVO_00000098 -->

    <owl:Class rdf:about="http://purl.obolibrary.org/obo/ENVO_00000098"/>
    


    <!-- http://purl.obolibrary.org/obo/ENVO_00000220 -->

    <owl:Class rdf:about="http://purl.obolibrary.org/obo/ENVO_00000220"/>
    


    <!-- http://purl.obolibrary.org/obo/ENVO_00000222 -->

    <owl:Class rdf:about="http://purl.obolibrary.org/obo/ENVO_00000222"/>
    


    <!-- http://purl.obolibrary.org/obo/ENVO_00000305 -->

    <owl:Class rdf:about="http://purl.obolibrary.org/obo/ENVO_00000305"/>
    


    <!-- http://purl.obolibrary.org/obo/ENVO_00000856 -->

    <owl:Class rdf:about="http://purl.obolibrary.org/obo/ENVO_00000856"/>
    


    <!-- http://purl.obolibrary.org/obo/GAZ_00009554 -->

    <owl:Class rdf:about="http://purl.obolibrary.org/obo/GAZ_00009554"/>
    


    <!-- http://purl.obolibrary.org/obo/GAZ_00009555 -->

    <owl:Class rdf:about="http://purl.obolibrary.org/obo/GAZ_00009555">
        <rdfs:subClassOf rdf:resource="http://purl.obolibrary.org/obo/GAZ_00009554"/>
    </owl:Class>
    


    <!-- http://purl.obolibrary.org/obo/GAZ_00009556 -->

    <owl:Class rdf:about="http://purl.obolibrary.org/obo/GAZ_00009556">
        <rdfs:subClassOf rdf:resource="http://purl.obolibrary.org/obo/GAZ_00009554"/>
    </owl:Class>
    


    <!-- http://purl.obolibrary.org/obo/GAZ_00009557 -->

    <owl:Class rdf:about="http://purl.obolibrary.org/obo/GAZ_00009557">
        <rdfs:subClassOf rdf:resource="http://purl.obolibrary.org/obo/GAZ_00009554"/>
    </owl:Class>
    


    <!-- http://purl.obolibrary.org/obo/GAZ_00009558 -->

    <owl:Class rdf:about="http://purl.obolibrary.org/obo/GAZ_00009558">
        <rdfs:subClassOf rdf:resource="http://purl.obolibrary.org/obo/GAZ_00009554"/>
    </owl:Class>
    


    <!-- http://purl.obolibrary.org/obo/GAZ_00012779 -->

    <owl:Class rdf:about="http://purl.obolibrary.org/obo/GAZ_00012779">
        <rdfs:subClassOf rdf:resource="http://purl.obolibrary.org/obo/GAZ_00009554"/>
    </owl:Class>
    


    <!-- http://purl.obolibrary.org/obo/GAZ_00012780 -->

    <owl:Class rdf:about="http://purl.obolibrary.org/obo/GAZ_00012780">
        <rdfs:subClassOf rdf:resource="http://purl.obolibrary.org/obo/GAZ_00009554"/>
    </owl:Class>
    


    <!-- http://purl.obolibrary.org/obo/GAZ_00012781 -->

    <owl:Class rdf:about="http://purl.obolibrary.org/obo/GAZ_00012781">
        <rdfs:subClassOf rdf:resource="http://purl.obolibrary.org/obo/GAZ_00009554"/>
    </owl:Class>
    


    <!-- http://purl.obolibrary.org/obo/GAZ_00012782 -->

    <owl:Class rdf:about="http://purl.obolibrary.org/obo/GAZ_00012782">
        <rdfs:subClassOf rdf:resource="http://purl.obolibrary.org/obo/GAZ_00009554"/>
    </owl:Class>
    


    <!-- http://purl.obolibrary.org/obo/GAZ_00012783 -->

    <owl:Class rdf:about="http://purl.obolibrary.org/obo/GAZ_00012783">
        <rdfs:subClassOf rdf:resource="http://purl.obolibrary.org/obo/GAZ_00009554"/>
    </owl:Class>
    


    <!-- 
    ///////////////////////////////////////////////////////////////////////////////////////
    //
    // Individuals
    //
    ///////////////////////////////////////////////////////////////////////////////////////
     -->

    


    <!-- http://purl.obolibrary.org/obo/GAZ_00001170 -->

    <owl:NamedIndividual rdf:about="http://purl.obolibrary.org/obo/GAZ_00001170">
        <rdf:type rdf:resource="http://purl.obolibrary.org/obo/ENVO_00000222"/>
        <obo:RO_0001025 rdf:resource="http://purl.obolibrary.org/obo/GAZ_00009557"/>
        <obo:IAO_0000115>A volcanic island in the southeastern part of the Solomon Islands province of Temotu. The island lies about 500 km to the east-southeast of Nendo.</obo:IAO_0000115>
        <oboInOwl:hasOBONamespace>GAZ</oboInOwl:hasOBONamespace>
        <oboInOwl:id>GAZ:00001170</oboInOwl:id>
        <rdfs:label>Anuta Island</rdfs:label>
    </owl:NamedIndividual>
    


    <!-- http://purl.obolibrary.org/obo/GAZ_00005275 -->

    <owl:NamedIndividual rdf:about="http://purl.obolibrary.org/obo/GAZ_00005275">
        <obo:IAO_0000115>A nation in Melanesia, east of Papua New Guinea, consisting of nearly one thousand islands. Together they cover a land mass of 28,400 km2. The capital is Honiara, located on the island of Guadalcanal.</obo:IAO_0000115>
        <oboInOwl:hasOBONamespace>GAZ</oboInOwl:hasOBONamespace>
        <oboInOwl:id>GAZ:00005275</oboInOwl:id>
        <rdfs:label>Solomon Islands</rdfs:label>
    </owl:NamedIndividual>
    


    <!-- http://purl.obolibrary.org/obo/GAZ_00005276 -->

    <owl:NamedIndividual rdf:about="http://purl.obolibrary.org/obo/GAZ_00005276">
        <obo:RO_0001025 rdf:resource="http://purl.obolibrary.org/obo/GAZ_00009555"/>
        <obo:IAO_0000115>An island in the Pacific Ocean.</obo:IAO_0000115>
        <oboInOwl:hasOBONamespace>GAZ</oboInOwl:hasOBONamespace>
        <oboInOwl:id>GAZ:00005276</oboInOwl:id>
        <rdfs:label>Guadalcanal</rdfs:label>
    </owl:NamedIndividual>
    


    <!-- http://purl.obolibrary.org/obo/GAZ_00007203 -->

    <owl:NamedIndividual rdf:about="http://purl.obolibrary.org/obo/GAZ_00007203">
        <obo:RO_0001025 rdf:resource="http://purl.obolibrary.org/obo/GAZ_00009558"/>
        <obo:IAO_0000115>The northernmost tract of land in the Solomon Islands, over 250 km north of Santa Isabel Island, and is an outlying part of Malaita Province. An atoll with over 122 small islets.</obo:IAO_0000115>
        <oboInOwl:hasOBONamespace>GAZ</oboInOwl:hasOBONamespace>
        <oboInOwl:id>GAZ:00007203</oboInOwl:id>
        <rdfs:label>Ontong Java Atoll</rdfs:label>
    </owl:NamedIndividual>
    


    <!-- http://purl.obolibrary.org/obo/GAZ_00007204 -->

    <owl:NamedIndividual rdf:about="http://purl.obolibrary.org/obo/GAZ_00007204">
        <obo:RO_0001025 rdf:resource="http://purl.obolibrary.org/obo/GAZ_00009557"/>
        <obo:IAO_0000115>A loose collection of islands in the northwestern part of the Solomon Islands province of Temotu. The islands lie about 80 km north of Nendo, the most important of the Santa Cruz Islands.</obo:IAO_0000115>
        <oboInOwl:hasOBONamespace>GAZ</oboInOwl:hasOBONamespace>
        <oboInOwl:id>GAZ:00007204</oboInOwl:id>
        <rdfs:label>Reef Islands</rdfs:label>
    </owl:NamedIndividual>
    


    <!-- http://purl.obolibrary.org/obo/GAZ_00007205 -->

    <owl:NamedIndividual rdf:about="http://purl.obolibrary.org/obo/GAZ_00007205">
        <obo:RO_0001025 rdf:resource="http://purl.obolibrary.org/obo/GAZ_00016939"/>
        <obo:IAO_0000115>An island in the Reef Islands, in the northern part of the Solomon Islands province of Temotu. Despite its location in Melanesia, the population of the islands is Polynesian.</obo:IAO_0000115>
        <oboInOwl:hasOBONamespace>GAZ</oboInOwl:hasOBONamespace>
        <oboInOwl:id>GAZ:00007205</oboInOwl:id>
        <rdfs:label>Pileni Island</rdfs:label>
    </owl:NamedIndividual>
    


    <!-- http://purl.obolibrary.org/obo/GAZ_00007206 -->

    <owl:NamedIndividual rdf:about="http://purl.obolibrary.org/obo/GAZ_00007206">
        <obo:RO_0001025 rdf:resource="http://purl.obolibrary.org/obo/GAZ_00009556"/>
        <obo:IAO_0000115>The largest island of Rennell and Bellona Province. It is almost totally surrounded by 120-150m cliffs and is comprised primarily of raised coral limestone, with the eastern end dominated by a brackish lake, Lake Te Nggano (also Lake Tegano), while the western end is relatively flat from the northern to southern coasts with rolling hills, (forested where not pasturalised), indicating its volcanic origins.</obo:IAO_0000115>
        <oboInOwl:hasOBONamespace>GAZ</oboInOwl:hasOBONamespace>
        <oboInOwl:id>GAZ:00007206</oboInOwl:id>
        <rdfs:label>Rennell Island</rdfs:label>
    </owl:NamedIndividual>
    


    <!-- http://purl.obolibrary.org/obo/GAZ_00007210 -->

    <owl:NamedIndividual rdf:about="http://purl.obolibrary.org/obo/GAZ_00007210">
        <obo:RO_0001025 rdf:resource="http://purl.obolibrary.org/obo/GAZ_00009557"/>
        <obo:IAO_0000115>A group of islands in the Pacific Ocean, part of Temotu Province of the Solomon Islands. They lie approximately 400 km to the southeast of the Solomon Islands Chain. The Santa Cruz Islands lie just north of the archipelago of Vanuatu, and are considered part of the Vanuatu rain forests ecoregion.</obo:IAO_0000115>
        <oboInOwl:hasOBONamespace>GAZ</oboInOwl:hasOBONamespace>
        <oboInOwl:id>GAZ:00007210</oboInOwl:id>
        <rdfs:label>Santa Cruz Islands</rdfs:label>
    </owl:NamedIndividual>
    


    <!-- http://purl.obolibrary.org/obo/GAZ_00007211 -->

    <owl:NamedIndividual rdf:about="http://purl.obolibrary.org/obo/GAZ_00007211">
        <obo:RO_0001025 rdf:resource="http://purl.obolibrary.org/obo/GAZ_00007210"/>
        <obo:IAO_0000115>The southernmost of the Santa Cruz Islands, located in the province of Temotu. It is also the southernmost of the Solomon Islands. Tikopia is a high island, covering an area of 5 km2. The island is the remnant of an extinct volcano, its highest point, Mt. Reani, reaching an elevation of 380 m above sea level.</obo:IAO_0000115>
        <oboInOwl:hasOBONamespace>GAZ</oboInOwl:hasOBONamespace>
        <oboInOwl:id>GAZ:00007211</oboInOwl:id>
        <rdfs:label>Tikopia Island</rdfs:label>
    </owl:NamedIndividual>
    


    <!-- http://purl.obolibrary.org/obo/GAZ_00009131 -->

    <owl:NamedIndividual rdf:about="http://purl.obolibrary.org/obo/GAZ_00009131">
        <obo:RO_0001025 rdf:resource="http://purl.obolibrary.org/obo/GAZ_00016910"/>
        <oboInOwl:hasOBONamespace>GAZ</oboInOwl:hasOBONamespace>
        <oboInOwl:id>GAZ:00009131</oboInOwl:id>
        <rdfs:label>Nggela Pile Island</rdfs:label>
    </owl:NamedIndividual>
    


    <!-- http://purl.obolibrary.org/obo/GAZ_00009132 -->

    <owl:NamedIndividual rdf:about="http://purl.obolibrary.org/obo/GAZ_00009132">
        <obo:RO_0001025 rdf:resource="http://purl.obolibrary.org/obo/GAZ_00012781"/>
        <obo:IAO_0000115>A group of islands belonging to the Western Province of the Solomon Islands, They lie in the extreme northwest of the country&apos;s territory, close to the island of Bougainville, Papua New Guinea.</obo:IAO_0000115>
        <oboInOwl:hasOBONamespace>GAZ</oboInOwl:hasOBONamespace>
        <oboInOwl:id>GAZ:00009132</oboInOwl:id>
        <rdfs:label>Shortland Islands</rdfs:label>
    </owl:NamedIndividual>
    


    <!-- http://purl.obolibrary.org/obo/GAZ_00009133 -->

    <owl:NamedIndividual rdf:about="http://purl.obolibrary.org/obo/GAZ_00009133">
        <obo:RO_0001025 rdf:resource="http://purl.obolibrary.org/obo/GAZ_00012781"/>
        <obo:IAO_0000115>A group of islands that are part of the Western Province of the Solomon Islands. They are located to the northwest of Guadalcanal.</obo:IAO_0000115>
        <oboInOwl:hasOBONamespace>GAZ</oboInOwl:hasOBONamespace>
        <oboInOwl:id>GAZ:00009133</oboInOwl:id>
        <rdfs:label>New Georgia Islands</rdfs:label>
    </owl:NamedIndividual>
    


    <!-- http://purl.obolibrary.org/obo/GAZ_00009134 -->

    <owl:NamedIndividual rdf:about="http://purl.obolibrary.org/obo/GAZ_00009134">
        <obo:RO_0001025 rdf:resource="http://purl.obolibrary.org/obo/GAZ_00012779"/>
        <obo:IAO_0000115>The largest island of Makira-Ulawa Province in the Solomon Islands. The island is located east of Guadalcanal and south of Malaita.</obo:IAO_0000115>
        <oboInOwl:hasOBONamespace>GAZ</oboInOwl:hasOBONamespace>
        <oboInOwl:id>GAZ:00009134</oboInOwl:id>
        <rdfs:label>Makira Island</rdfs:label>
    </owl:NamedIndividual>
    


    <!-- http://purl.obolibrary.org/obo/GAZ_00009135 -->

    <owl:NamedIndividual rdf:about="http://purl.obolibrary.org/obo/GAZ_00009135">
        <obo:RO_0001025 rdf:resource="http://purl.obolibrary.org/obo/GAZ_00012783"/>
        <obo:IAO_0000115>Two small islands, as well as several islets, of volcanic origin, in the Central Province of the Solomon Islands. They are located approximately 48 km northwest from Guadalcanal.</obo:IAO_0000115>
        <oboInOwl:hasOBONamespace>GAZ</oboInOwl:hasOBONamespace>
        <oboInOwl:id>GAZ:00009135</oboInOwl:id>
        <rdfs:label>Russell Islands</rdfs:label>
    </owl:NamedIndividual>
    


    <!-- http://purl.obolibrary.org/obo/GAZ_00009136 -->

    <owl:NamedIndividual rdf:about="http://purl.obolibrary.org/obo/GAZ_00009136">
        <obo:RO_0001025 rdf:resource="http://purl.obolibrary.org/obo/GAZ_00012782"/>
        <obo:IAO_0000115>The longest in the Solomon Islands, South Pacific, and the largest in Isabel Province. Choiseul lies to the west, Malaita to the east. The Pacific Ocean lies to the north, and the Slot to the south.</obo:IAO_0000115>
        <oboInOwl:hasOBONamespace>GAZ</oboInOwl:hasOBONamespace>
        <oboInOwl:id>GAZ:00009136</oboInOwl:id>
        <rdfs:label>Santa Isabel Island</rdfs:label>
    </owl:NamedIndividual>
    


    <!-- http://purl.obolibrary.org/obo/GAZ_00009137 -->

    <owl:NamedIndividual rdf:about="http://purl.obolibrary.org/obo/GAZ_00009137">
        <obo:RO_0001025 rdf:resource="http://purl.obolibrary.org/obo/GAZ_00009558"/>
        <obo:IAO_0000115>The largest island of the Malaita Province in the Solomon Islands.</obo:IAO_0000115>
        <oboInOwl:hasOBONamespace>GAZ</oboInOwl:hasOBONamespace>
        <oboInOwl:id>GAZ:00009137</oboInOwl:id>
        <rdfs:label>Malaita Island</rdfs:label>
    </owl:NamedIndividual>
    


    <!-- http://purl.obolibrary.org/obo/GAZ_00009138 -->

    <owl:NamedIndividual rdf:about="http://purl.obolibrary.org/obo/GAZ_00009138">
        <obo:RO_0001025 rdf:resource="http://purl.obolibrary.org/obo/GAZ_00012780"/>
        <obo:IAO_0000115>The largest island (2,971 km2) of the Choiseul Province, Solomon Islands.</obo:IAO_0000115>
        <oboInOwl:hasOBONamespace>GAZ</oboInOwl:hasOBONamespace>
        <oboInOwl:id>GAZ:00009138</oboInOwl:id>
        <rdfs:label>Choiseul Island</rdfs:label>
    </owl:NamedIndividual>
    


    <!-- http://purl.obolibrary.org/obo/GAZ_00009139 -->

    <owl:NamedIndividual rdf:about="http://purl.obolibrary.org/obo/GAZ_00009139">
        <obo:RO_0001025 rdf:resource="http://purl.obolibrary.org/obo/GAZ_00012779"/>
        <obo:IAO_0000115>An island in the Solomon Islands; it is located in Makira-Ulawa Province.</obo:IAO_0000115>
        <oboInOwl:hasOBONamespace>GAZ</oboInOwl:hasOBONamespace>
        <oboInOwl:id>GAZ:00009139</oboInOwl:id>
        <rdfs:label>Uki Island</rdfs:label>
    </owl:NamedIndividual>
    


    <!-- http://purl.obolibrary.org/obo/GAZ_00009143 -->

    <owl:NamedIndividual rdf:about="http://purl.obolibrary.org/obo/GAZ_00009143">
        <obo:RO_0001025 rdf:resource="http://purl.obolibrary.org/obo/GAZ_00012779"/>
        <obo:IAO_0000115>A coral island in the Solomon Islands; it is located in Makira-Ulawa Province.</obo:IAO_0000115>
        <oboInOwl:hasOBONamespace>GAZ</oboInOwl:hasOBONamespace>
        <oboInOwl:id>GAZ:00009143</oboInOwl:id>
        <rdfs:label>Owaraha Island</rdfs:label>
    </owl:NamedIndividual>
    


    <!-- http://purl.obolibrary.org/obo/GAZ_00009146 -->

    <owl:NamedIndividual rdf:about="http://purl.obolibrary.org/obo/GAZ_00009146">
        <rdf:type rdf:resource="http://purl.obolibrary.org/obo/ENVO_00000222"/>
        <obo:RO_0001025 rdf:resource="http://purl.obolibrary.org/obo/GAZ_00009557"/>
        <obo:IAO_0000115>A volcanic island in the Solomon Islands province of Temotu.</obo:IAO_0000115>
        <oboInOwl:hasOBONamespace>GAZ</oboInOwl:hasOBONamespace>
        <oboInOwl:id>GAZ:00009146</oboInOwl:id>
        <rdfs:label>Fatutaka Island</rdfs:label>
    </owl:NamedIndividual>
    


    <!-- http://purl.obolibrary.org/obo/GAZ_00009554 -->

    <owl:NamedIndividual rdf:about="http://purl.obolibrary.org/obo/GAZ_00009554">
        <obo:RO_0001025 rdf:resource="http://purl.obolibrary.org/obo/GAZ_00005275"/>
    </owl:NamedIndividual>
    


    <!-- http://purl.obolibrary.org/obo/GAZ_00009555 -->

    <owl:NamedIndividual rdf:about="http://purl.obolibrary.org/obo/GAZ_00009555"/>
    


    <!-- http://purl.obolibrary.org/obo/GAZ_00009556 -->

    <owl:NamedIndividual rdf:about="http://purl.obolibrary.org/obo/GAZ_00009556"/>
    


    <!-- http://purl.obolibrary.org/obo/GAZ_00009557 -->

    <owl:NamedIndividual rdf:about="http://purl.obolibrary.org/obo/GAZ_00009557"/>
    


    <!-- http://purl.obolibrary.org/obo/GAZ_00009558 -->

    <owl:NamedIndividual rdf:about="http://purl.obolibrary.org/obo/GAZ_00009558"/>
    


    <!-- http://purl.obolibrary.org/obo/GAZ_00012779 -->

    <owl:NamedIndividual rdf:about="http://purl.obolibrary.org/obo/GAZ_00012779"/>
    


    <!-- http://purl.obolibrary.org/obo/GAZ_00012780 -->

    <owl:NamedIndividual rdf:about="http://purl.obolibrary.org/obo/GAZ_00012780"/>
    


    <!-- http://purl.obolibrary.org/obo/GAZ_00012781 -->

    <owl:NamedIndividual rdf:about="http://purl.obolibrary.org/obo/GAZ_00012781"/>
    


    <!-- http://purl.obolibrary.org/obo/GAZ_00012782 -->

    <owl:NamedIndividual rdf:about="http://purl.obolibrary.org/obo/GAZ_00012782"/>
    


    <!-- http://purl.obolibrary.org/obo/GAZ_00012783 -->

    <owl:NamedIndividual rdf:about="http://purl.obolibrary.org/obo/GAZ_00012783"/>
    


    <!-- http://purl.obolibrary.org/obo/GAZ_00016882 -->

    <owl:NamedIndividual rdf:about="http://purl.obolibrary.org/obo/GAZ_00016882">
        <obo:RO_0001025 rdf:resource="http://purl.obolibrary.org/obo/GAZ_00012780"/>
        <obo:IAO_0000115>An island in the Solomon Islands; it is located in Choiseul Province.</obo:IAO_0000115>
        <oboInOwl:hasOBONamespace>GAZ</oboInOwl:hasOBONamespace>
        <oboInOwl:id>GAZ:00016882</oboInOwl:id>
        <rdfs:label>Taro Island</rdfs:label>
    </owl:NamedIndividual>
    


    <!-- http://purl.obolibrary.org/obo/GAZ_00016883 -->

    <owl:NamedIndividual rdf:about="http://purl.obolibrary.org/obo/GAZ_00016883">
        <obo:RO_0001025 rdf:resource="http://purl.obolibrary.org/obo/GAZ_00009132"/>
        <obo:IAO_0000115>An island.</obo:IAO_0000115>
        <oboInOwl:hasOBONamespace>GAZ</oboInOwl:hasOBONamespace>
        <oboInOwl:id>GAZ:00016883</oboInOwl:id>
        <rdfs:label>Pirumeri Island</rdfs:label>
    </owl:NamedIndividual>
    


    <!-- http://purl.obolibrary.org/obo/GAZ_00016884 -->

    <owl:NamedIndividual rdf:about="http://purl.obolibrary.org/obo/GAZ_00016884">
        <obo:RO_0001025 rdf:resource="http://purl.obolibrary.org/obo/GAZ_00009132"/>
        <obo:IAO_0000115>An island.</obo:IAO_0000115>
        <oboInOwl:hasOBONamespace>GAZ</oboInOwl:hasOBONamespace>
        <oboInOwl:id>GAZ:00016884</oboInOwl:id>
        <rdfs:label>Magusaiai Island</rdfs:label>
    </owl:NamedIndividual>
    


    <!-- http://purl.obolibrary.org/obo/GAZ_00016885 -->

    <owl:NamedIndividual rdf:about="http://purl.obolibrary.org/obo/GAZ_00016885">
        <obo:RO_0001025 rdf:resource="http://purl.obolibrary.org/obo/GAZ_00009132"/>
        <obo:IAO_0000115>An island.</obo:IAO_0000115>
        <oboInOwl:hasOBONamespace>GAZ</oboInOwl:hasOBONamespace>
        <oboInOwl:id>GAZ:00016885</oboInOwl:id>
        <rdfs:label>Ovau Island</rdfs:label>
    </owl:NamedIndividual>
    


    <!-- http://purl.obolibrary.org/obo/GAZ_00016886 -->

    <owl:NamedIndividual rdf:about="http://purl.obolibrary.org/obo/GAZ_00016886">
        <obo:RO_0001025 rdf:resource="http://purl.obolibrary.org/obo/GAZ_00009132"/>
        <oboInOwl:hasOBONamespace>GAZ</oboInOwl:hasOBONamespace>
        <oboInOwl:id>GAZ:00016886</oboInOwl:id>
        <rdfs:label>Alu Island</rdfs:label>
    </owl:NamedIndividual>
    


    <!-- http://purl.obolibrary.org/obo/GAZ_00016887 -->

    <owl:NamedIndividual rdf:about="http://purl.obolibrary.org/obo/GAZ_00016887">
        <obo:RO_0001025 rdf:resource="http://purl.obolibrary.org/obo/GAZ_00009132"/>
        <obo:IAO_0000115>An island.</obo:IAO_0000115>
        <oboInOwl:hasOBONamespace>GAZ</oboInOwl:hasOBONamespace>
        <oboInOwl:id>GAZ:00016887</oboInOwl:id>
        <rdfs:label>Masamasa Island</rdfs:label>
    </owl:NamedIndividual>
    


    <!-- http://purl.obolibrary.org/obo/GAZ_00016888 -->

    <owl:NamedIndividual rdf:about="http://purl.obolibrary.org/obo/GAZ_00016888">
        <obo:RO_0001025 rdf:resource="http://purl.obolibrary.org/obo/GAZ_00009132"/>
        <obo:IAO_0000115>An island, one of the Shortland Islands, Solomon Islands.</obo:IAO_0000115>
        <oboInOwl:hasOBONamespace>GAZ</oboInOwl:hasOBONamespace>
        <oboInOwl:id>GAZ:00016888</oboInOwl:id>
        <rdfs:label>Fauro Island</rdfs:label>
    </owl:NamedIndividual>
    


    <!-- http://purl.obolibrary.org/obo/GAZ_00016889 -->

    <owl:NamedIndividual rdf:about="http://purl.obolibrary.org/obo/GAZ_00016889">
        <obo:RO_0001025 rdf:resource="http://purl.obolibrary.org/obo/GAZ_00012781"/>
        <obo:IAO_0000115>A small group of islands a few km to the south of Bougainville and 24 km from the Shortland Islands. They form part of the Western Province of the Solomon Islands.</obo:IAO_0000115>
        <oboInOwl:hasOBONamespace>GAZ</oboInOwl:hasOBONamespace>
        <oboInOwl:id>GAZ:00016889</oboInOwl:id>
        <rdfs:label>Treasury Islands</rdfs:label>
    </owl:NamedIndividual>
    


    <!-- http://purl.obolibrary.org/obo/GAZ_00016890 -->

    <owl:NamedIndividual rdf:about="http://purl.obolibrary.org/obo/GAZ_00016890">
        <obo:RO_0001025 rdf:resource="http://purl.obolibrary.org/obo/GAZ_00016889"/>
        <obo:IAO_0000115>The largest island of the Treasury Islands, Solomon Islands.</obo:IAO_0000115>
        <oboInOwl:hasOBONamespace>GAZ</oboInOwl:hasOBONamespace>
        <oboInOwl:id>GAZ:00016890</oboInOwl:id>
        <rdfs:label>Mono Island</rdfs:label>
    </owl:NamedIndividual>
    


    <!-- http://purl.obolibrary.org/obo/GAZ_00016891 -->

    <owl:NamedIndividual rdf:about="http://purl.obolibrary.org/obo/GAZ_00016891">
        <obo:RO_0001025 rdf:resource="http://purl.obolibrary.org/obo/GAZ_00016889"/>
        <obo:IAO_0000115>The smaller island of the Treasury Islands, Solomon Islands.</obo:IAO_0000115>
        <oboInOwl:hasOBONamespace>GAZ</oboInOwl:hasOBONamespace>
        <oboInOwl:id>GAZ:00016891</oboInOwl:id>
        <rdfs:label>Stirling Island</rdfs:label>
    </owl:NamedIndividual>
    


    <!-- http://purl.obolibrary.org/obo/GAZ_00016892 -->

    <owl:NamedIndividual rdf:about="http://purl.obolibrary.org/obo/GAZ_00016892">
        <obo:RO_0001025 rdf:resource="http://purl.obolibrary.org/obo/GAZ_00009133"/>
        <obo:IAO_0000115>An island.</obo:IAO_0000115>
        <oboInOwl:hasOBONamespace>GAZ</oboInOwl:hasOBONamespace>
        <oboInOwl:id>GAZ:00016892</oboInOwl:id>
        <rdfs:label>Tetepare Island</rdfs:label>
    </owl:NamedIndividual>
    


    <!-- http://purl.obolibrary.org/obo/GAZ_00016893 -->

    <owl:NamedIndividual rdf:about="http://purl.obolibrary.org/obo/GAZ_00016893">
        <rdf:type rdf:resource="http://purl.obolibrary.org/obo/ENVO_00000222"/>
        <obo:RO_0001025 rdf:resource="http://purl.obolibrary.org/obo/GAZ_00009133"/>
        <obo:IAO_0000115>A volcanic island.</obo:IAO_0000115>
        <oboInOwl:hasOBONamespace>GAZ</oboInOwl:hasOBONamespace>
        <oboInOwl:id>GAZ:00016893</oboInOwl:id>
        <rdfs:label>Mborokua Island</rdfs:label>
    </owl:NamedIndividual>
    


    <!-- http://purl.obolibrary.org/obo/GAZ_00016894 -->

    <owl:NamedIndividual rdf:about="http://purl.obolibrary.org/obo/GAZ_00016894">
        <rdf:type rdf:resource="http://purl.obolibrary.org/obo/ENVO_00000222"/>
        <obo:RO_0001025 rdf:resource="http://purl.obolibrary.org/obo/GAZ_00009133"/>
        <obo:IAO_0000115>A volcanic island in the Solomon Islands; it is located in the Western Province.</obo:IAO_0000115>
        <oboInOwl:hasOBONamespace>GAZ</oboInOwl:hasOBONamespace>
        <oboInOwl:id>GAZ:00016894</oboInOwl:id>
        <rdfs:label>Vangunu Island</rdfs:label>
    </owl:NamedIndividual>
    


    <!-- http://purl.obolibrary.org/obo/GAZ_00016895 -->

    <owl:NamedIndividual rdf:about="http://purl.obolibrary.org/obo/GAZ_00016895">
        <obo:RO_0001025 rdf:resource="http://purl.obolibrary.org/obo/GAZ_00009133"/>
        <obo:IAO_0000115>An island, part of the New Georgia Islands, Solomon Islands.</obo:IAO_0000115>
        <oboInOwl:hasOBONamespace>GAZ</oboInOwl:hasOBONamespace>
        <oboInOwl:id>GAZ:00016895</oboInOwl:id>
        <rdfs:label>Rendova Island</rdfs:label>
    </owl:NamedIndividual>
    


    <!-- http://purl.obolibrary.org/obo/GAZ_00016896 -->

    <owl:NamedIndividual rdf:about="http://purl.obolibrary.org/obo/GAZ_00016896">
        <obo:RO_0001025 rdf:resource="http://purl.obolibrary.org/obo/GAZ_00016899"/>
        <obo:IAO_0000115>A populated place.</obo:IAO_0000115>
        <oboInOwl:hasOBONamespace>GAZ</oboInOwl:hasOBONamespace>
        <oboInOwl:id>GAZ:00016896</oboInOwl:id>
        <rdfs:label>Penjuku</rdfs:label>
    </owl:NamedIndividual>
    


    <!-- http://purl.obolibrary.org/obo/GAZ_00016897 -->

    <owl:NamedIndividual rdf:about="http://purl.obolibrary.org/obo/GAZ_00016897">
        <obo:RO_0001025 rdf:resource="http://purl.obolibrary.org/obo/GAZ_00009133"/>
        <oboInOwl:hasOBONamespace>GAZ</oboInOwl:hasOBONamespace>
        <oboInOwl:id>GAZ:00016897</oboInOwl:id>
        <rdfs:label>Akara Island</rdfs:label>
    </owl:NamedIndividual>
    


    <!-- http://purl.obolibrary.org/obo/GAZ_00016898 -->

    <owl:NamedIndividual rdf:about="http://purl.obolibrary.org/obo/GAZ_00016898">
        <obo:RO_0001025 rdf:resource="http://purl.obolibrary.org/obo/GAZ_00009133"/>
        <obo:IAO_0000115>The largest island of the Western Province of the Solomon Islands. It is in the New Georgia Group, an archipelago including most of the other larger islands in the province.</obo:IAO_0000115>
        <oboInOwl:hasOBONamespace>GAZ</oboInOwl:hasOBONamespace>
        <oboInOwl:id>GAZ:00016898</oboInOwl:id>
        <rdfs:label>New Georgia Island</rdfs:label>
    </owl:NamedIndividual>
    


    <!-- http://purl.obolibrary.org/obo/GAZ_00016899 -->

    <owl:NamedIndividual rdf:about="http://purl.obolibrary.org/obo/GAZ_00016899">
        <rdf:type rdf:resource="http://purl.obolibrary.org/obo/ENVO_00000222"/>
        <obo:RO_0001025 rdf:resource="http://purl.obolibrary.org/obo/GAZ_00009133"/>
        <obo:IAO_0000115>A volcanic island in the New Georgia Islands group of Solomon Islands.</obo:IAO_0000115>
        <oboInOwl:hasOBONamespace>GAZ</oboInOwl:hasOBONamespace>
        <oboInOwl:id>GAZ:00016899</oboInOwl:id>
        <rdfs:label>Nggatokae Island</rdfs:label>
    </owl:NamedIndividual>
    


    <!-- http://purl.obolibrary.org/obo/GAZ_00016900 -->

    <owl:NamedIndividual rdf:about="http://purl.obolibrary.org/obo/GAZ_00016900">
        <obo:RO_0001025 rdf:resource="http://purl.obolibrary.org/obo/GAZ_00009133"/>
        <obo:IAO_0000115>An island in the Solomon Islands; it is located in the Western Province.</obo:IAO_0000115>
        <oboInOwl:hasOBONamespace>GAZ</oboInOwl:hasOBONamespace>
        <oboInOwl:id>GAZ:00016900</oboInOwl:id>
        <rdfs:label>Mbava Island</rdfs:label>
    </owl:NamedIndividual>
    


    <!-- http://purl.obolibrary.org/obo/GAZ_00016901 -->

    <owl:NamedIndividual rdf:about="http://purl.obolibrary.org/obo/GAZ_00016901">
        <obo:RO_0001025 rdf:resource="http://purl.obolibrary.org/obo/GAZ_00009133"/>
        <obo:IAO_0000115>An island in the Solomon Islands; it is located in the Western Province.</obo:IAO_0000115>
        <oboInOwl:hasOBONamespace>GAZ</oboInOwl:hasOBONamespace>
        <oboInOwl:id>GAZ:00016901</oboInOwl:id>
        <rdfs:label>Kohinggo Island</rdfs:label>
    </owl:NamedIndividual>
    


    <!-- http://purl.obolibrary.org/obo/GAZ_00016902 -->

    <owl:NamedIndividual rdf:about="http://purl.obolibrary.org/obo/GAZ_00016902">
        <obo:RO_0001025 rdf:resource="http://purl.obolibrary.org/obo/GAZ_00009133"/>
        <obo:IAO_0000115>An island.</obo:IAO_0000115>
        <oboInOwl:hasOBONamespace>GAZ</oboInOwl:hasOBONamespace>
        <oboInOwl:id>GAZ:00016902</oboInOwl:id>
        <rdfs:label>Ghizo Island</rdfs:label>
    </owl:NamedIndividual>
    


    <!-- http://purl.obolibrary.org/obo/GAZ_00016903 -->

    <owl:NamedIndividual rdf:about="http://purl.obolibrary.org/obo/GAZ_00016903">
        <obo:RO_0001025 rdf:resource="http://purl.obolibrary.org/obo/GAZ_00009133"/>
        <obo:IAO_0000115>An island in the Western Province of the Solomon Islands. It lies to the west of New Georgia, but is considered one of the New Georgia Group. To its west is the Treasury Islands.</obo:IAO_0000115>
        <oboInOwl:hasOBONamespace>GAZ</oboInOwl:hasOBONamespace>
        <oboInOwl:id>GAZ:00016903</oboInOwl:id>
        <rdfs:label>Vella Lavella Island</rdfs:label>
    </owl:NamedIndividual>
    


    <!-- http://purl.obolibrary.org/obo/GAZ_00016904 -->

    <owl:NamedIndividual rdf:about="http://purl.obolibrary.org/obo/GAZ_00016904">
        <obo:RO_0001025 rdf:resource="http://purl.obolibrary.org/obo/GAZ_00009133"/>
        <obo:IAO_0000115>An island located in the New Georgia Islands group of Western Province, Solomon Islands.</obo:IAO_0000115>
        <oboInOwl:hasOBONamespace>GAZ</oboInOwl:hasOBONamespace>
        <oboInOwl:id>GAZ:00016904</oboInOwl:id>
        <rdfs:label>Ranongga Island</rdfs:label>
    </owl:NamedIndividual>
    


    <!-- http://purl.obolibrary.org/obo/GAZ_00016905 -->

    <owl:NamedIndividual rdf:about="http://purl.obolibrary.org/obo/GAZ_00016905">
        <obo:RO_0001025 rdf:resource="http://purl.obolibrary.org/obo/GAZ_00009133"/>
        <obo:IAO_0000115>An island with three truncated andesitic volcanic centers. The only Potassium-Argon date (2.3 +/- 1 million years ago from Mount Patukio) suggests a Pliocene-to-Pleistocene age for the island (Solomon Islands Geological Survey, 1982). The southern half of the island is thermally active. It contains fault-related fumarolic areas and hot springs near saltwater Lake Ove along the western coast and along the eastern coast near Mount Patukio, which has a steep-walled summit crater. Grover (1955) noted native accounts of the explosive enlargement of the Ngusunu explosion crater along the SW coast of the island one to two generations prior to 1955, probably after a visit by Guppy in 1882. Press reports mentioned an eruption at Simbo in the early 1900s that forced the evacuation of villages beside Lake Ove, immediately adjacent to Ngusunu crater.</obo:IAO_0000115>
        <oboInOwl:hasOBONamespace>GAZ</oboInOwl:hasOBONamespace>
        <oboInOwl:id>GAZ:00016905</oboInOwl:id>
        <rdfs:label>Simbo Island</rdfs:label>
    </owl:NamedIndividual>
    


    <!-- http://purl.obolibrary.org/obo/GAZ_00016906 -->

    <owl:NamedIndividual rdf:about="http://purl.obolibrary.org/obo/GAZ_00016906">
        <obo:RO_0001025 rdf:resource="http://purl.obolibrary.org/obo/GAZ_00009133"/>
        <obo:IAO_0000115>An island in the Solomon Islands; it is located in the Western Province.</obo:IAO_0000115>
        <oboInOwl:hasOBONamespace>GAZ</oboInOwl:hasOBONamespace>
        <oboInOwl:id>GAZ:00016906</oboInOwl:id>
        <rdfs:label>Vonavona Island</rdfs:label>
    </owl:NamedIndividual>
    


    <!-- http://purl.obolibrary.org/obo/GAZ_00016907 -->

    <owl:NamedIndividual rdf:about="http://purl.obolibrary.org/obo/GAZ_00016907">
        <obo:RO_0001025 rdf:resource="http://purl.obolibrary.org/obo/GAZ_00009133"/>
        <obo:IAO_0000115>An island in the New Georgia Islands group of the Solomon Islands.</obo:IAO_0000115>
        <oboInOwl:hasOBONamespace>GAZ</oboInOwl:hasOBONamespace>
        <oboInOwl:id>GAZ:00016907</oboInOwl:id>
        <rdfs:label>Kolombangara Island</rdfs:label>
    </owl:NamedIndividual>
    


    <!-- http://purl.obolibrary.org/obo/GAZ_00016908 -->

    <owl:NamedIndividual rdf:about="http://purl.obolibrary.org/obo/GAZ_00016908">
        <obo:RO_0001025 rdf:resource="http://purl.obolibrary.org/obo/GAZ_00012782"/>
        <obo:IAO_0000115>The second largest island in the Isabel Province, Solomon Islands.</obo:IAO_0000115>
        <oboInOwl:hasOBONamespace>GAZ</oboInOwl:hasOBONamespace>
        <oboInOwl:id>GAZ:00016908</oboInOwl:id>
        <rdfs:label>San Jorge Island</rdfs:label>
    </owl:NamedIndividual>
    


    <!-- http://purl.obolibrary.org/obo/GAZ_00016909 -->

    <owl:NamedIndividual rdf:about="http://purl.obolibrary.org/obo/GAZ_00016909">
        <obo:RO_0001025 rdf:resource="http://purl.obolibrary.org/obo/GAZ_00009135"/>
        <obo:IAO_0000115>The largest of the Russell Islands in Central Province, Solomon Islands. It is located Northwest of Guadalcanal.</obo:IAO_0000115>
        <oboInOwl:hasOBONamespace>GAZ</oboInOwl:hasOBONamespace>
        <oboInOwl:id>GAZ:00016909</oboInOwl:id>
        <rdfs:label>Pavuvu Island</rdfs:label>
    </owl:NamedIndividual>
    


    <!-- http://purl.obolibrary.org/obo/GAZ_00016910 -->

    <owl:NamedIndividual rdf:about="http://purl.obolibrary.org/obo/GAZ_00016910">
        <rdf:type rdf:resource="http://purl.obolibrary.org/obo/ENVO_00000220"/>
        <obo:RO_0001025 rdf:resource="http://purl.obolibrary.org/obo/GAZ_00012783"/>
        <obo:IAO_0000115>A small island group in the Central Province of the Solomon Islands, a nation in the western Pacific Ocean.</obo:IAO_0000115>
        <oboInOwl:hasOBONamespace>GAZ</oboInOwl:hasOBONamespace>
        <oboInOwl:id>GAZ:00016910</oboInOwl:id>
        <rdfs:label>Florida Islands</rdfs:label>
    </owl:NamedIndividual>
    


    <!-- http://purl.obolibrary.org/obo/GAZ_00016911 -->

    <owl:NamedIndividual rdf:about="http://purl.obolibrary.org/obo/GAZ_00016911">
        <obo:RO_0001025 rdf:resource="http://purl.obolibrary.org/obo/GAZ_00016910"/>
        <obo:IAO_0000115>A small island (5.5 km by 1 km) in the Solomon Islands, just off the south coast of Florida Island.</obo:IAO_0000115>
        <oboInOwl:hasOBONamespace>GAZ</oboInOwl:hasOBONamespace>
        <oboInOwl:id>GAZ:00016911</oboInOwl:id>
        <rdfs:label>Tulagi Island</rdfs:label>
    </owl:NamedIndividual>
    


    <!-- http://purl.obolibrary.org/obo/GAZ_00016912 -->

    <owl:NamedIndividual rdf:about="http://purl.obolibrary.org/obo/GAZ_00016912">
        <obo:RO_0001025 rdf:resource="http://purl.obolibrary.org/obo/GAZ_00016910"/>
        <oboInOwl:hasOBONamespace>GAZ</oboInOwl:hasOBONamespace>
        <oboInOwl:id>GAZ:00016912</oboInOwl:id>
        <rdfs:label>Nggela Sule Island</rdfs:label>
    </owl:NamedIndividual>
    


    <!-- http://purl.obolibrary.org/obo/GAZ_00016913 -->

    <owl:NamedIndividual rdf:about="http://purl.obolibrary.org/obo/GAZ_00016913">
        <obo:RO_0001025 rdf:resource="http://purl.obolibrary.org/obo/GAZ_00016910"/>
        <obo:IAO_0000115>An island in the Central Province of the Solomon Islands. It is one of the Florida Islands.</obo:IAO_0000115>
        <oboInOwl:hasOBONamespace>GAZ</oboInOwl:hasOBONamespace>
        <oboInOwl:id>GAZ:00016913</oboInOwl:id>
        <rdfs:label>Tanambogo Island</rdfs:label>
    </owl:NamedIndividual>
    


    <!-- http://purl.obolibrary.org/obo/GAZ_00016914 -->

    <owl:NamedIndividual rdf:about="http://purl.obolibrary.org/obo/GAZ_00016914">
        <obo:RO_0001025 rdf:resource="http://purl.obolibrary.org/obo/GAZ_00016910"/>
        <obo:IAO_0000115>A small island in the Central Province of the Solomon Islands.</obo:IAO_0000115>
        <oboInOwl:hasOBONamespace>GAZ</oboInOwl:hasOBONamespace>
        <oboInOwl:id>GAZ:00016914</oboInOwl:id>
        <rdfs:label>Gavutu Island</rdfs:label>
    </owl:NamedIndividual>
    


    <!-- http://purl.obolibrary.org/obo/GAZ_00016915 -->

    <owl:NamedIndividual rdf:about="http://purl.obolibrary.org/obo/GAZ_00016915">
        <obo:RO_0001025 rdf:resource="http://purl.obolibrary.org/obo/GAZ_00009558"/>
        <obo:IAO_0000115>An atoll.</obo:IAO_0000115>
        <oboInOwl:hasOBONamespace>GAZ</oboInOwl:hasOBONamespace>
        <oboInOwl:id>GAZ:00016915</oboInOwl:id>
        <rdfs:label>Sikaiana Atoll</rdfs:label>
    </owl:NamedIndividual>
    


    <!-- http://purl.obolibrary.org/obo/GAZ_00016917 -->

    <owl:NamedIndividual rdf:about="http://purl.obolibrary.org/obo/GAZ_00016917">
        <obo:RO_0001025 rdf:resource="http://purl.obolibrary.org/obo/GAZ_00016915"/>
        <obo:IAO_0000115>An island.</obo:IAO_0000115>
        <oboInOwl:hasOBONamespace>GAZ</oboInOwl:hasOBONamespace>
        <oboInOwl:id>GAZ:00016917</oboInOwl:id>
        <rdfs:label>Mutuavi Island</rdfs:label>
    </owl:NamedIndividual>
    


    <!-- http://purl.obolibrary.org/obo/GAZ_00016918 -->

    <owl:NamedIndividual rdf:about="http://purl.obolibrary.org/obo/GAZ_00016918">
        <obo:RO_0001025 rdf:resource="http://purl.obolibrary.org/obo/GAZ_00009558"/>
        <obo:IAO_0000115>An island W of Sikaiana Atoll.</obo:IAO_0000115>
        <oboInOwl:hasOBONamespace>GAZ</oboInOwl:hasOBONamespace>
        <oboInOwl:id>GAZ:00016918</oboInOwl:id>
        <rdfs:label>Faore Island</rdfs:label>
    </owl:NamedIndividual>
    


    <!-- http://purl.obolibrary.org/obo/GAZ_00016919 -->

    <owl:NamedIndividual rdf:about="http://purl.obolibrary.org/obo/GAZ_00016919">
        <obo:RO_0001025 rdf:resource="http://purl.obolibrary.org/obo/GAZ_00009558"/>
        <obo:IAO_0000115>A reef in the Solomon Islands, south of Ontong Java Atoll and north of Santa Isabel Island.</obo:IAO_0000115>
        <oboInOwl:hasOBONamespace>GAZ</oboInOwl:hasOBONamespace>
        <oboInOwl:id>GAZ:00016919</oboInOwl:id>
        <rdfs:label>Roncador Reef</rdfs:label>
    </owl:NamedIndividual>
    


    <!-- http://purl.obolibrary.org/obo/GAZ_00016920 -->

    <owl:NamedIndividual rdf:about="http://purl.obolibrary.org/obo/GAZ_00016920">
        <obo:RO_0001025 rdf:resource="http://purl.obolibrary.org/obo/GAZ_00009558"/>
        <oboInOwl:hasOBONamespace>GAZ</oboInOwl:hasOBONamespace>
        <oboInOwl:id>GAZ:00016920</oboInOwl:id>
        <rdfs:label>Olu Malau Islands</rdfs:label>
    </owl:NamedIndividual>
    


    <!-- http://purl.obolibrary.org/obo/GAZ_00016921 -->

    <owl:NamedIndividual rdf:about="http://purl.obolibrary.org/obo/GAZ_00016921">
        <obo:RO_0001025 rdf:resource="http://purl.obolibrary.org/obo/GAZ_00016920"/>
        <oboInOwl:hasOBONamespace>GAZ</oboInOwl:hasOBONamespace>
        <oboInOwl:id>GAZ:00016921</oboInOwl:id>
        <rdfs:label>Malaulo Island</rdfs:label>
    </owl:NamedIndividual>
    


    <!-- http://purl.obolibrary.org/obo/GAZ_00016922 -->

    <owl:NamedIndividual rdf:about="http://purl.obolibrary.org/obo/GAZ_00016922">
        <obo:RO_0001025 rdf:resource="http://purl.obolibrary.org/obo/GAZ_00016920"/>
        <oboInOwl:hasOBONamespace>GAZ</oboInOwl:hasOBONamespace>
        <oboInOwl:id>GAZ:00016922</oboInOwl:id>
        <rdfs:label>Malaupaina Island</rdfs:label>
    </owl:NamedIndividual>
    


    <!-- http://purl.obolibrary.org/obo/GAZ_00016923 -->

    <owl:NamedIndividual rdf:about="http://purl.obolibrary.org/obo/GAZ_00016923">
        <obo:RO_0001025 rdf:resource="http://purl.obolibrary.org/obo/GAZ_00016920"/>
        <oboInOwl:hasOBONamespace>GAZ</oboInOwl:hasOBONamespace>
        <oboInOwl:id>GAZ:00016923</oboInOwl:id>
        <rdfs:label>Ali Ite Island</rdfs:label>
    </owl:NamedIndividual>
    


    <!-- http://purl.obolibrary.org/obo/GAZ_00016927 -->

    <owl:NamedIndividual rdf:about="http://purl.obolibrary.org/obo/GAZ_00016927">
        <obo:RO_0001025 rdf:resource="http://purl.obolibrary.org/obo/GAZ_00012779"/>
        <obo:IAO_0000115>An island in the Solomon Islands. It is located near Malaita Island and belongs to Makira Province.</obo:IAO_0000115>
        <oboInOwl:hasOBONamespace>GAZ</oboInOwl:hasOBONamespace>
        <oboInOwl:id>GAZ:00016927</oboInOwl:id>
        <rdfs:label>Ulawa Island</rdfs:label>
    </owl:NamedIndividual>
    


    <!-- http://purl.obolibrary.org/obo/GAZ_00016929 -->

    <owl:NamedIndividual rdf:about="http://purl.obolibrary.org/obo/GAZ_00016929">
        <obo:RO_0001025 rdf:resource="http://purl.obolibrary.org/obo/GAZ_00009556"/>
        <obo:IAO_0000115>An island of the Rennell and Bellona Province, Solomon Islands.</obo:IAO_0000115>
        <oboInOwl:hasOBONamespace>GAZ</oboInOwl:hasOBONamespace>
        <oboInOwl:id>GAZ:00016929</oboInOwl:id>
        <rdfs:label>Bellona Island</rdfs:label>
    </owl:NamedIndividual>
    


    <!-- http://purl.obolibrary.org/obo/GAZ_00016930 -->

    <owl:NamedIndividual rdf:about="http://purl.obolibrary.org/obo/GAZ_00016930">
        <obo:RO_0001025 rdf:resource="http://purl.obolibrary.org/obo/GAZ_00007210"/>
        <obo:IAO_0000115>The exposed summit of a massive stratovolcano that rises 3-4 km from the sea floor at the NW end of the Santa Cruz islands. Tinakula resembles Stromboli volcano in containing a breached summit crater that extends from the 851 m high summit to below sea level. Landslides enlarged this scarp in 1965, creating an embayment on the NW coast. The satellitic cone of Mendana is located on the SE side. The dominantly andesitic Tinakula volcano has frequently been observed in eruption since the era of Spanish exploration began in 1595. In about 1840, an explosive eruption apparently produced pyroclastic flows that swept all sides of the island, killing its inhabitants. Frequent historical eruptions have originated from a cone constructed within the large breached crater. These have left the upper flanks of the volcano and the steep apron of lava flows and volcaniclastic debris within the breach unvegetated.</obo:IAO_0000115>
        <oboInOwl:hasOBONamespace>GAZ</oboInOwl:hasOBONamespace>
        <oboInOwl:id>GAZ:00016930</oboInOwl:id>
        <rdfs:label>Tinakula Island</rdfs:label>
    </owl:NamedIndividual>
    


    <!-- http://purl.obolibrary.org/obo/GAZ_00016931 -->

    <owl:NamedIndividual rdf:about="http://purl.obolibrary.org/obo/GAZ_00016931">
        <rdf:type rdf:resource="http://purl.obolibrary.org/obo/ENVO_00000220"/>
        <obo:RO_0001025 rdf:resource="http://purl.obolibrary.org/obo/GAZ_00007210"/>
        <obo:IAO_0000115>An island group.</obo:IAO_0000115>
        <oboInOwl:hasOBONamespace>GAZ</oboInOwl:hasOBONamespace>
        <oboInOwl:id>GAZ:00016931</oboInOwl:id>
        <rdfs:label>Nendo Islands</rdfs:label>
    </owl:NamedIndividual>
    


    <!-- http://purl.obolibrary.org/obo/GAZ_00016932 -->

    <owl:NamedIndividual rdf:about="http://purl.obolibrary.org/obo/GAZ_00016932">
        <obo:RO_0001025 rdf:resource="http://purl.obolibrary.org/obo/GAZ_00007210"/>
        <obo:IAO_0000115>A group of several nearby islands surrounded by a single belt of coral reef.</obo:IAO_0000115>
        <oboInOwl:hasOBONamespace>GAZ</oboInOwl:hasOBONamespace>
        <oboInOwl:id>GAZ:00016932</oboInOwl:id>
        <rdfs:label>Vanikolo Islands</rdfs:label>
    </owl:NamedIndividual>
    


    <!-- http://purl.obolibrary.org/obo/GAZ_00016933 -->

    <owl:NamedIndividual rdf:about="http://purl.obolibrary.org/obo/GAZ_00016933">
        <obo:RO_0001025 rdf:resource="http://purl.obolibrary.org/obo/GAZ_00007210"/>
        <obo:IAO_0000115>An island located 66 km to the Southeast of the main Santa Cruz group, between Vanikoro and Santa Cruz proper.</obo:IAO_0000115>
        <oboInOwl:hasOBONamespace>GAZ</oboInOwl:hasOBONamespace>
        <oboInOwl:id>GAZ:00016933</oboInOwl:id>
        <rdfs:label>Utupua Island</rdfs:label>
    </owl:NamedIndividual>
    


    <!-- http://purl.obolibrary.org/obo/GAZ_00016934 -->

    <owl:NamedIndividual rdf:about="http://purl.obolibrary.org/obo/GAZ_00016934">
        <obo:RO_0001025 rdf:resource="http://purl.obolibrary.org/obo/GAZ_00016932"/>
        <obo:IAO_0000115>An island.</obo:IAO_0000115>
        <oboInOwl:hasOBONamespace>GAZ</oboInOwl:hasOBONamespace>
        <oboInOwl:id>GAZ:00016934</oboInOwl:id>
        <rdfs:label>Banie Island</rdfs:label>
    </owl:NamedIndividual>
    


    <!-- http://purl.obolibrary.org/obo/GAZ_00016935 -->

    <owl:NamedIndividual rdf:about="http://purl.obolibrary.org/obo/GAZ_00016935">
        <obo:RO_0001025 rdf:resource="http://purl.obolibrary.org/obo/GAZ_00016932"/>
        <obo:IAO_0000115>An island.</obo:IAO_0000115>
        <oboInOwl:hasOBONamespace>GAZ</oboInOwl:hasOBONamespace>
        <oboInOwl:id>GAZ:00016935</oboInOwl:id>
        <rdfs:label>Tevai Island</rdfs:label>
    </owl:NamedIndividual>
    


    <!-- http://purl.obolibrary.org/obo/GAZ_00016936 -->

    <owl:NamedIndividual rdf:about="http://purl.obolibrary.org/obo/GAZ_00016936">
        <obo:RO_0001025 rdf:resource="http://purl.obolibrary.org/obo/GAZ_00016931"/>
        <obo:IAO_0000115>A satellite island of Nendo Island.</obo:IAO_0000115>
        <oboInOwl:hasOBONamespace>GAZ</oboInOwl:hasOBONamespace>
        <oboInOwl:id>GAZ:00016936</oboInOwl:id>
        <rdfs:label>Malo Island</rdfs:label>
    </owl:NamedIndividual>
    


    <!-- http://purl.obolibrary.org/obo/GAZ_00016937 -->

    <owl:NamedIndividual rdf:about="http://purl.obolibrary.org/obo/GAZ_00016937">
        <obo:RO_0001025 rdf:resource="http://purl.obolibrary.org/obo/GAZ_00016931"/>
        <obo:IAO_0000115>A satellite island of Nendo Island.</obo:IAO_0000115>
        <oboInOwl:hasOBONamespace>GAZ</oboInOwl:hasOBONamespace>
        <oboInOwl:id>GAZ:00016937</oboInOwl:id>
        <rdfs:label>Nibanga Island</rdfs:label>
    </owl:NamedIndividual>
    


    <!-- http://purl.obolibrary.org/obo/GAZ_00016938 -->

    <owl:NamedIndividual rdf:about="http://purl.obolibrary.org/obo/GAZ_00016938">
        <obo:RO_0001025 rdf:resource="http://purl.obolibrary.org/obo/GAZ_00016931"/>
        <obo:IAO_0000115>The largest, and most important of the Santa Cruz Islands, located in the Temotu province of the Solomon Islands.</obo:IAO_0000115>
        <oboInOwl:hasOBONamespace>GAZ</oboInOwl:hasOBONamespace>
        <oboInOwl:id>GAZ:00016938</oboInOwl:id>
        <rdfs:label>Nendo Island</rdfs:label>
    </owl:NamedIndividual>
    


    <!-- http://purl.obolibrary.org/obo/GAZ_00016939 -->

    <owl:NamedIndividual rdf:about="http://purl.obolibrary.org/obo/GAZ_00016939">
        <obo:RO_0001025 rdf:resource="http://purl.obolibrary.org/obo/GAZ_00007204"/>
        <oboInOwl:hasOBONamespace>GAZ</oboInOwl:hasOBONamespace>
        <oboInOwl:id>GAZ:00016939</oboInOwl:id>
        <rdfs:label>Outer Islands</rdfs:label>
    </owl:NamedIndividual>
    


    <!-- http://purl.obolibrary.org/obo/GAZ_00016940 -->

    <owl:NamedIndividual rdf:about="http://purl.obolibrary.org/obo/GAZ_00016940">
        <obo:RO_0001025 rdf:resource="http://purl.obolibrary.org/obo/GAZ_00016939"/>
        <obo:IAO_0000115>An outer reef in the Reef Islands, in the Solomon Islands province of Temotu. It is located about 50 km northeast of Nupani.</obo:IAO_0000115>
        <oboInOwl:hasOBONamespace>GAZ</oboInOwl:hasOBONamespace>
        <oboInOwl:id>GAZ:00016940</oboInOwl:id>
        <rdfs:label>Patteson Shoal</rdfs:label>
    </owl:NamedIndividual>
    


    <!-- http://purl.obolibrary.org/obo/GAZ_00016941 -->

    <owl:NamedIndividual rdf:about="http://purl.obolibrary.org/obo/GAZ_00016941">
        <obo:RO_0001025 rdf:resource="http://purl.obolibrary.org/obo/GAZ_00016939"/>
        <obo:IAO_0000115>An island in the Reef Islands, in the Solomon Islands province of Temotu.</obo:IAO_0000115>
        <oboInOwl:hasOBONamespace>GAZ</oboInOwl:hasOBONamespace>
        <oboInOwl:id>GAZ:00016941</oboInOwl:id>
        <rdfs:label>Makalom Island</rdfs:label>
    </owl:NamedIndividual>
    


    <!-- http://purl.obolibrary.org/obo/GAZ_00016942 -->

    <owl:NamedIndividual rdf:about="http://purl.obolibrary.org/obo/GAZ_00016942">
        <obo:RO_0001025 rdf:resource="http://purl.obolibrary.org/obo/GAZ_00016939"/>
        <obo:IAO_0000115>An atoll.</obo:IAO_0000115>
        <oboInOwl:hasOBONamespace>GAZ</oboInOwl:hasOBONamespace>
        <oboInOwl:id>GAZ:00016942</oboInOwl:id>
        <rdfs:label>Nupani Island</rdfs:label>
    </owl:NamedIndividual>
    


    <!-- http://purl.obolibrary.org/obo/GAZ_00016943 -->

    <owl:NamedIndividual rdf:about="http://purl.obolibrary.org/obo/GAZ_00016943">
        <obo:RO_0001025 rdf:resource="http://purl.obolibrary.org/obo/GAZ_00016939"/>
        <obo:IAO_0000115>An atoll.</obo:IAO_0000115>
        <oboInOwl:hasOBONamespace>GAZ</oboInOwl:hasOBONamespace>
        <oboInOwl:id>GAZ:00016943</oboInOwl:id>
        <rdfs:label>Nalongo Island</rdfs:label>
    </owl:NamedIndividual>
    


    <!-- http://purl.obolibrary.org/obo/GAZ_00016944 -->

    <owl:NamedIndividual rdf:about="http://purl.obolibrary.org/obo/GAZ_00016944">
        <obo:RO_0001025 rdf:resource="http://purl.obolibrary.org/obo/GAZ_00007204"/>
        <obo:IAO_0000115>A continuous shoal, extending about 25 km west of Nifiloli.</obo:IAO_0000115>
        <oboInOwl:hasOBONamespace>GAZ</oboInOwl:hasOBONamespace>
        <oboInOwl:id>GAZ:00016944</oboInOwl:id>
        <rdfs:label>Numa Miombilou</rdfs:label>
    </owl:NamedIndividual>
    


    <!-- http://purl.obolibrary.org/obo/GAZ_00016945 -->

    <owl:NamedIndividual rdf:about="http://purl.obolibrary.org/obo/GAZ_00016945">
        <obo:RO_0001025 rdf:resource="http://purl.obolibrary.org/obo/GAZ_00016939"/>
        <obo:IAO_0000115>An atoll. Located to the Northwest of the main Reef Islands separated from them by approximately 20 km of ocean.</obo:IAO_0000115>
        <oboInOwl:hasOBONamespace>GAZ</oboInOwl:hasOBONamespace>
        <oboInOwl:id>GAZ:00016945</oboInOwl:id>
        <rdfs:label>Nukapu Island</rdfs:label>
    </owl:NamedIndividual>
    


    <!-- http://purl.obolibrary.org/obo/GAZ_00016946 -->

    <owl:NamedIndividual rdf:about="http://purl.obolibrary.org/obo/GAZ_00016946">
        <obo:RO_0001025 rdf:resource="http://purl.obolibrary.org/obo/GAZ_00007204"/>
        <obo:IAO_0000115>A coral reef.</obo:IAO_0000115>
        <oboInOwl:hasOBONamespace>GAZ</oboInOwl:hasOBONamespace>
        <oboInOwl:id>GAZ:00016946</oboInOwl:id>
        <rdfs:label>Malim Reef</rdfs:label>
    </owl:NamedIndividual>
    


    <!-- http://purl.obolibrary.org/obo/GAZ_00016947 -->

    <owl:NamedIndividual rdf:about="http://purl.obolibrary.org/obo/GAZ_00016947">
        <obo:RO_0001025 rdf:resource="http://purl.obolibrary.org/obo/GAZ_00007204"/>
        <obo:IAO_0000115>A coral reef.</obo:IAO_0000115>
        <oboInOwl:hasOBONamespace>GAZ</oboInOwl:hasOBONamespace>
        <oboInOwl:id>GAZ:00016947</oboInOwl:id>
        <rdfs:label>Manuwa Reef</rdfs:label>
    </owl:NamedIndividual>
    


    <!-- http://purl.obolibrary.org/obo/GAZ_00016948 -->

    <owl:NamedIndividual rdf:about="http://purl.obolibrary.org/obo/GAZ_00016948">
        <obo:RO_0001025 rdf:resource="http://purl.obolibrary.org/obo/GAZ_00007204"/>
        <obo:IAO_0000115>A coral reef.</obo:IAO_0000115>
        <oboInOwl:hasOBONamespace>GAZ</oboInOwl:hasOBONamespace>
        <oboInOwl:id>GAZ:00016948</oboInOwl:id>
        <rdfs:label>Malani Reef</rdfs:label>
    </owl:NamedIndividual>
    


    <!-- http://purl.obolibrary.org/obo/GAZ_00016949 -->

    <owl:NamedIndividual rdf:about="http://purl.obolibrary.org/obo/GAZ_00016949">
        <obo:RO_0001025 rdf:resource="http://purl.obolibrary.org/obo/GAZ_00007204"/>
        <obo:IAO_0000115>A coral reef.</obo:IAO_0000115>
        <oboInOwl:hasOBONamespace>GAZ</oboInOwl:hasOBONamespace>
        <oboInOwl:id>GAZ:00016949</oboInOwl:id>
        <rdfs:label>Matumbi Reef</rdfs:label>
    </owl:NamedIndividual>
    


    <!-- http://purl.obolibrary.org/obo/GAZ_00016950 -->

    <owl:NamedIndividual rdf:about="http://purl.obolibrary.org/obo/GAZ_00016950">
        <obo:RO_0001025 rdf:resource="http://purl.obolibrary.org/obo/GAZ_00007204"/>
        <oboInOwl:hasOBONamespace>GAZ</oboInOwl:hasOBONamespace>
        <oboInOwl:id>GAZ:00016950</oboInOwl:id>
        <rdfs:label>Grimbanga Nende Atoll</rdfs:label>
    </owl:NamedIndividual>
    


    <!-- http://purl.obolibrary.org/obo/GAZ_00016951 -->

    <owl:NamedIndividual rdf:about="http://purl.obolibrary.org/obo/GAZ_00016951">
        <obo:RO_0001025 rdf:resource="http://purl.obolibrary.org/obo/GAZ_00007204"/>
        <obo:IAO_0000115>One of the Reef Islands, of the independent nation of the Solomon Islands; it is located in Temotu Province.</obo:IAO_0000115>
        <oboInOwl:hasOBONamespace>GAZ</oboInOwl:hasOBONamespace>
        <oboInOwl:id>GAZ:00016951</oboInOwl:id>
        <rdfs:label>Matema Island</rdfs:label>
    </owl:NamedIndividual>
    


    <!-- http://purl.obolibrary.org/obo/GAZ_00016952 -->

    <owl:NamedIndividual rdf:about="http://purl.obolibrary.org/obo/GAZ_00016952">
        <obo:RO_0001025 rdf:resource="http://purl.obolibrary.org/obo/GAZ_00007204"/>
        <obo:IAO_0000115>An island in the Solomon Islands; it is located in Temotu Province.</obo:IAO_0000115>
        <oboInOwl:hasOBONamespace>GAZ</oboInOwl:hasOBONamespace>
        <oboInOwl:id>GAZ:00016952</oboInOwl:id>
        <rdfs:label>Pigeon Island</rdfs:label>
    </owl:NamedIndividual>
    


    <!-- http://purl.obolibrary.org/obo/GAZ_00016953 -->

    <owl:NamedIndividual rdf:about="http://purl.obolibrary.org/obo/GAZ_00016953">
        <obo:RO_0001025 rdf:resource="http://purl.obolibrary.org/obo/GAZ_00007204"/>
        <oboInOwl:hasOBONamespace>GAZ</oboInOwl:hasOBONamespace>
        <oboInOwl:id>GAZ:00016953</oboInOwl:id>
        <rdfs:label>Grimbanga Temoa Atoll</rdfs:label>
    </owl:NamedIndividual>
    


    <!-- http://purl.obolibrary.org/obo/GAZ_00016954 -->

    <owl:NamedIndividual rdf:about="http://purl.obolibrary.org/obo/GAZ_00016954">
        <obo:RO_0001025 rdf:resource="http://purl.obolibrary.org/obo/GAZ_00007204"/>
        <oboInOwl:hasOBONamespace>GAZ</oboInOwl:hasOBONamespace>
        <oboInOwl:id>GAZ:00016954</oboInOwl:id>
        <rdfs:label>Ngatendo Atoll</rdfs:label>
    </owl:NamedIndividual>
    


    <!-- http://purl.obolibrary.org/obo/GAZ_00016955 -->

    <owl:NamedIndividual rdf:about="http://purl.obolibrary.org/obo/GAZ_00016955">
        <obo:RO_0001025 rdf:resource="http://purl.obolibrary.org/obo/GAZ_00007204"/>
        <obo:IAO_0000115>An island in the Reef Islands, in the of the Solomon Islands province of Temotu.</obo:IAO_0000115>
        <oboInOwl:hasOBONamespace>GAZ</oboInOwl:hasOBONamespace>
        <oboInOwl:id>GAZ:00016955</oboInOwl:id>
        <rdfs:label>Nifiloli Atoll</rdfs:label>
    </owl:NamedIndividual>
    


    <!-- http://purl.obolibrary.org/obo/GAZ_00016956 -->

    <owl:NamedIndividual rdf:about="http://purl.obolibrary.org/obo/GAZ_00016956">
        <obo:RO_0001025 rdf:resource="http://purl.obolibrary.org/obo/GAZ_00007204"/>
        <oboInOwl:hasOBONamespace>GAZ</oboInOwl:hasOBONamespace>
        <oboInOwl:id>GAZ:00016956</oboInOwl:id>
        <rdfs:label>Ngawa Atoll</rdfs:label>
    </owl:NamedIndividual>
    


    <!-- http://purl.obolibrary.org/obo/GAZ_00016957 -->

    <owl:NamedIndividual rdf:about="http://purl.obolibrary.org/obo/GAZ_00016957">
        <obo:RO_0001025 rdf:resource="http://purl.obolibrary.org/obo/GAZ_00007204"/>
        <obo:IAO_0000115>The second largest island in the Reef Islands, administratively located in the Solomon Islands province of Temotu. At low tide, Fenualoa is connected to the neighboring island of Nifiloli to the north.</obo:IAO_0000115>
        <oboInOwl:hasOBONamespace>GAZ</oboInOwl:hasOBONamespace>
        <oboInOwl:id>GAZ:00016957</oboInOwl:id>
        <rdfs:label>Fenualoa Atoll</rdfs:label>
    </owl:NamedIndividual>
    


    <!-- http://purl.obolibrary.org/obo/GAZ_00016958 -->

    <owl:NamedIndividual rdf:about="http://purl.obolibrary.org/obo/GAZ_00016958">
        <obo:RO_0001025 rdf:resource="http://purl.obolibrary.org/obo/GAZ_00007204"/>
        <oboInOwl:hasOBONamespace>GAZ</oboInOwl:hasOBONamespace>
        <oboInOwl:id>GAZ:00016958</oboInOwl:id>
        <rdfs:label>Ngandeli Atoll</rdfs:label>
    </owl:NamedIndividual>
    


    <!-- http://purl.obolibrary.org/obo/GAZ_00016959 -->

    <owl:NamedIndividual rdf:about="http://purl.obolibrary.org/obo/GAZ_00016959">
        <obo:RO_0001025 rdf:resource="http://purl.obolibrary.org/obo/GAZ_00007204"/>
        <obo:IAO_0000115>An atoll.</obo:IAO_0000115>
        <oboInOwl:hasOBONamespace>GAZ</oboInOwl:hasOBONamespace>
        <oboInOwl:id>GAZ:00016959</oboInOwl:id>
        <rdfs:label>Ngalo Atoll</rdfs:label>
    </owl:NamedIndividual>
    


    <!-- http://purl.obolibrary.org/obo/GAZ_00016960 -->

    <owl:NamedIndividual rdf:about="http://purl.obolibrary.org/obo/GAZ_00016960">
        <obo:RO_0001025 rdf:resource="http://purl.obolibrary.org/obo/GAZ_00009557"/>
        <obo:IAO_0000115>A small island group lying to the northeast of the Santa Cruz Islands in the Solomon Islands province of Temotu.</obo:IAO_0000115>
        <oboInOwl:hasOBONamespace>GAZ</oboInOwl:hasOBONamespace>
        <oboInOwl:id>GAZ:00016960</oboInOwl:id>
        <rdfs:label>Duff Islands</rdfs:label>
    </owl:NamedIndividual>
    


    <!-- http://purl.obolibrary.org/obo/GAZ_00016961 -->

    <owl:NamedIndividual rdf:about="http://purl.obolibrary.org/obo/GAZ_00016961">
        <rdf:type rdf:resource="http://purl.obolibrary.org/obo/ENVO_00000220"/>
        <obo:RO_0001025 rdf:resource="http://purl.obolibrary.org/obo/GAZ_00016960"/>
        <obo:IAO_0000115>An island group.</obo:IAO_0000115>
        <oboInOwl:hasOBONamespace>GAZ</oboInOwl:hasOBONamespace>
        <oboInOwl:id>GAZ:00016961</oboInOwl:id>
        <rdfs:label>Taumako Islands</rdfs:label>
    </owl:NamedIndividual>
    


    <!-- http://purl.obolibrary.org/obo/GAZ_00016962 -->

    <owl:NamedIndividual rdf:about="http://purl.obolibrary.org/obo/GAZ_00016962">
        <obo:RO_0001025 rdf:resource="http://purl.obolibrary.org/obo/GAZ_00016961"/>
        <obo:IAO_0000115>An island.</obo:IAO_0000115>
        <oboInOwl:hasOBONamespace>GAZ</oboInOwl:hasOBONamespace>
        <oboInOwl:id>GAZ:00016962</oboInOwl:id>
        <rdfs:label>Tahua Island</rdfs:label>
    </owl:NamedIndividual>
    


    <!-- http://purl.obolibrary.org/obo/GAZ_00016963 -->

    <owl:NamedIndividual rdf:about="http://purl.obolibrary.org/obo/GAZ_00016963">
        <obo:RO_0001025 rdf:resource="http://purl.obolibrary.org/obo/GAZ_00016961"/>
        <obo:IAO_0000115>An island.</obo:IAO_0000115>
        <oboInOwl:hasOBONamespace>GAZ</oboInOwl:hasOBONamespace>
        <oboInOwl:id>GAZ:00016963</oboInOwl:id>
        <rdfs:label>Tohua Island</rdfs:label>
    </owl:NamedIndividual>
    


    <!-- http://purl.obolibrary.org/obo/GAZ_00016964 -->

    <owl:NamedIndividual rdf:about="http://purl.obolibrary.org/obo/GAZ_00016964">
        <obo:RO_0001025 rdf:resource="http://purl.obolibrary.org/obo/GAZ_00016961"/>
        <obo:IAO_0000115>The largest of the Duff Islands.</obo:IAO_0000115>
        <oboInOwl:hasOBONamespace>GAZ</oboInOwl:hasOBONamespace>
        <oboInOwl:id>GAZ:00016964</oboInOwl:id>
        <rdfs:label>Taumako Island</rdfs:label>
    </owl:NamedIndividual>
    


    <!-- http://purl.obolibrary.org/obo/GAZ_00016965 -->

    <owl:NamedIndividual rdf:about="http://purl.obolibrary.org/obo/GAZ_00016965">
        <rdf:type rdf:resource="http://purl.obolibrary.org/obo/ENVO_00000220"/>
        <obo:RO_0001025 rdf:resource="http://purl.obolibrary.org/obo/GAZ_00016960"/>
        <obo:IAO_0000115>An island group.</obo:IAO_0000115>
        <oboInOwl:hasOBONamespace>GAZ</oboInOwl:hasOBONamespace>
        <oboInOwl:id>GAZ:00016965</oboInOwl:id>
        <rdfs:label>Bass Islands</rdfs:label>
    </owl:NamedIndividual>
    


    <!-- http://purl.obolibrary.org/obo/GAZ_00016966 -->

    <owl:NamedIndividual rdf:about="http://purl.obolibrary.org/obo/GAZ_00016966">
        <obo:RO_0001025 rdf:resource="http://purl.obolibrary.org/obo/GAZ_00016965"/>
        <obo:IAO_0000115>An island.</obo:IAO_0000115>
        <oboInOwl:hasOBONamespace>GAZ</oboInOwl:hasOBONamespace>
        <oboInOwl:id>GAZ:00016966</oboInOwl:id>
        <rdfs:label>Kaa Island</rdfs:label>
    </owl:NamedIndividual>
    


    <!-- http://purl.obolibrary.org/obo/GAZ_00016967 -->

    <owl:NamedIndividual rdf:about="http://purl.obolibrary.org/obo/GAZ_00016967">
        <obo:RO_0001025 rdf:resource="http://purl.obolibrary.org/obo/GAZ_00016965"/>
        <obo:IAO_0000115>An island.</obo:IAO_0000115>
        <oboInOwl:hasOBONamespace>GAZ</oboInOwl:hasOBONamespace>
        <oboInOwl:id>GAZ:00016967</oboInOwl:id>
        <rdfs:label>Lua Island</rdfs:label>
    </owl:NamedIndividual>
    


    <!-- http://purl.obolibrary.org/obo/GAZ_00016968 -->

    <owl:NamedIndividual rdf:about="http://purl.obolibrary.org/obo/GAZ_00016968">
        <obo:RO_0001025 rdf:resource="http://purl.obolibrary.org/obo/GAZ_00016965"/>
        <obo:IAO_0000115>An island.</obo:IAO_0000115>
        <oboInOwl:hasOBONamespace>GAZ</oboInOwl:hasOBONamespace>
        <oboInOwl:id>GAZ:00016968</oboInOwl:id>
        <rdfs:label>Loreva Island</rdfs:label>
    </owl:NamedIndividual>
    


    <!-- http://purl.obolibrary.org/obo/GAZ_00016969 -->

    <owl:NamedIndividual rdf:about="http://purl.obolibrary.org/obo/GAZ_00016969">
        <rdf:type rdf:resource="http://purl.obolibrary.org/obo/ENVO_00000220"/>
        <obo:RO_0001025 rdf:resource="http://purl.obolibrary.org/obo/GAZ_00016960"/>
        <obo:IAO_0000115>An island group.</obo:IAO_0000115>
        <oboInOwl:hasOBONamespace>GAZ</oboInOwl:hasOBONamespace>
        <oboInOwl:id>GAZ:00016969</oboInOwl:id>
        <rdfs:label>Treasurer&apos;s Islands</rdfs:label>
    </owl:NamedIndividual>
    


    <!-- http://purl.obolibrary.org/obo/GAZ_00016970 -->

    <owl:NamedIndividual rdf:about="http://purl.obolibrary.org/obo/GAZ_00016970">
        <obo:RO_0001025 rdf:resource="http://purl.obolibrary.org/obo/GAZ_00016969"/>
        <obo:IAO_0000115>An island.</obo:IAO_0000115>
        <oboInOwl:hasOBONamespace>GAZ</oboInOwl:hasOBONamespace>
        <oboInOwl:id>GAZ:00016970</oboInOwl:id>
        <rdfs:label>Lakao Island</rdfs:label>
    </owl:NamedIndividual>
    


    <!-- http://purl.obolibrary.org/obo/GAZ_00016971 -->

    <owl:NamedIndividual rdf:about="http://purl.obolibrary.org/obo/GAZ_00016971">
        <obo:RO_0001025 rdf:resource="http://purl.obolibrary.org/obo/GAZ_00016969"/>
        <obo:IAO_0000115>An island.</obo:IAO_0000115>
        <oboInOwl:hasOBONamespace>GAZ</oboInOwl:hasOBONamespace>
        <oboInOwl:id>GAZ:00016971</oboInOwl:id>
        <rdfs:label>Ulaka Island</rdfs:label>
    </owl:NamedIndividual>
    


    <!-- http://purl.obolibrary.org/obo/GAZ_00016972 -->

    <owl:NamedIndividual rdf:about="http://purl.obolibrary.org/obo/GAZ_00016972">
        <obo:RO_0001025 rdf:resource="http://purl.obolibrary.org/obo/GAZ_00016969"/>
        <obo:IAO_0000115>An island.</obo:IAO_0000115>
        <oboInOwl:hasOBONamespace>GAZ</oboInOwl:hasOBONamespace>
        <oboInOwl:id>GAZ:00016972</oboInOwl:id>
        <rdfs:label>Tuleki Island</rdfs:label>
    </owl:NamedIndividual>
    


    <!-- http://purl.obolibrary.org/obo/GAZ_00016973 -->

    <owl:NamedIndividual rdf:about="http://purl.obolibrary.org/obo/GAZ_00016973">
        <obo:RO_0001025 rdf:resource="http://purl.obolibrary.org/obo/GAZ_00016969"/>
        <obo:IAO_0000115>An island.</obo:IAO_0000115>
        <oboInOwl:hasOBONamespace>GAZ</oboInOwl:hasOBONamespace>
        <oboInOwl:id>GAZ:00016973</oboInOwl:id>
        <rdfs:label>Te Aku Island</rdfs:label>
    </owl:NamedIndividual>
    


    <!-- http://purl.obolibrary.org/obo/GAZ_00016974 -->

    <owl:NamedIndividual rdf:about="http://purl.obolibrary.org/obo/GAZ_00016974">
        <obo:RO_0001025 rdf:resource="http://purl.obolibrary.org/obo/GAZ_00016960"/>
        <obo:IAO_0000115>A reef.</obo:IAO_0000115>
        <oboInOwl:hasOBONamespace>GAZ</oboInOwl:hasOBONamespace>
        <oboInOwl:id>GAZ:00016974</oboInOwl:id>
        <rdfs:label>Hallie Jackson Reef</rdfs:label>
    </owl:NamedIndividual>
    


    <!-- http://purl.obolibrary.org/obo/GAZ_00049011 -->

    <owl:NamedIndividual rdf:about="http://purl.obolibrary.org/obo/GAZ_00049011">
        <obo:RO_0001025 rdf:resource="http://purl.obolibrary.org/obo/GAZ_00007203"/>
        <oboInOwl:hasOBONamespace>GAZ</oboInOwl:hasOBONamespace>
        <oboInOwl:id>GAZ:00049011</oboInOwl:id>
        <rdfs:label>Luaniua Island</rdfs:label>
    </owl:NamedIndividual>
    


    <!-- http://purl.obolibrary.org/obo/GAZ_00049012 -->

    <owl:NamedIndividual rdf:about="http://purl.obolibrary.org/obo/GAZ_00049012">
        <obo:RO_0001025 rdf:resource="http://purl.obolibrary.org/obo/GAZ_00007203"/>
        <oboInOwl:hasOBONamespace>GAZ</oboInOwl:hasOBONamespace>
        <oboInOwl:id>GAZ:00049012</oboInOwl:id>
        <rdfs:label>Pelau Island</rdfs:label>
    </owl:NamedIndividual>
    


    <!-- http://purl.obolibrary.org/obo/GAZ_00049013 -->

    <owl:NamedIndividual rdf:about="http://purl.obolibrary.org/obo/GAZ_00049013">
        <obo:RO_0001025 rdf:resource="http://purl.obolibrary.org/obo/GAZ_00007203"/>
        <oboInOwl:hasOBONamespace>GAZ</oboInOwl:hasOBONamespace>
        <oboInOwl:id>GAZ:00049013</oboInOwl:id>
        <rdfs:label>Kemalu Island</rdfs:label>
    </owl:NamedIndividual>
    


    <!-- http://purl.obolibrary.org/obo/GAZ_00049014 -->

    <owl:NamedIndividual rdf:about="http://purl.obolibrary.org/obo/GAZ_00049014">
        <obo:RO_0001025 rdf:resource="http://purl.obolibrary.org/obo/GAZ_00012779"/>
        <obo:IAO_0000115>A coral island in the Solomon Islands; it is located in Makira-Ulawa Province.</obo:IAO_0000115>
        <oboInOwl:hasOBONamespace>GAZ</oboInOwl:hasOBONamespace>
        <oboInOwl:id>GAZ:00049014</oboInOwl:id>
        <rdfs:label>Owariki Island</rdfs:label>
    </owl:NamedIndividual>
    


    <!-- http://purl.obolibrary.org/obo/GAZ_00049015 -->

    <owl:NamedIndividual rdf:about="http://purl.obolibrary.org/obo/GAZ_00049015">
        <obo:RO_0001025 rdf:resource="http://purl.obolibrary.org/obo/GAZ_00012783"/>
        <obo:IAO_0000115>An island that consists of a forested andesitic-to-dacitic stratovolcano with a shallow, elliptical 1 x 1.5 km wide summit crater. Lava domes of historical age are located on the crater floor and its NE rim, and older domes occur on the flanks of the volcano. Pyroclastic flows and mudflows traveled down valleys from the summit crater to form debris fans along the coast. Thermal areas located in the summit crater, the south to SE flanks, and offshore include areas of steaming ground, fumaroles, small geysers, and hot springs. Spanish explorers arrived in 1568 during the first historical eruption of Savo. Pyroclastic flows during the climactic phase killed almost all inhabitants of the island, and oral traditions also note the expansion of the island on the northern side.</obo:IAO_0000115>
        <oboInOwl:hasOBONamespace>GAZ</oboInOwl:hasOBONamespace>
        <oboInOwl:id>GAZ:00049015</oboInOwl:id>
        <rdfs:label>Savo Island</rdfs:label>
    </owl:NamedIndividual>
    


    <!-- http://purl.obolibrary.org/obo/GAZ_00049016 -->

    <owl:NamedIndividual rdf:about="http://purl.obolibrary.org/obo/GAZ_00049016">
        <obo:RO_0001025 rdf:resource="http://purl.obolibrary.org/obo/GAZ_00012780"/>
        <obo:IAO_0000115>An island in the Solomon Islands; it is located in Choiseul Province.</obo:IAO_0000115>
        <oboInOwl:hasOBONamespace>GAZ</oboInOwl:hasOBONamespace>
        <oboInOwl:id>GAZ:00049016</oboInOwl:id>
        <rdfs:label>Rob Roy Island</rdfs:label>
    </owl:NamedIndividual>
    


    <!-- http://purl.obolibrary.org/obo/GAZ_00049017 -->

    <owl:NamedIndividual rdf:about="http://purl.obolibrary.org/obo/GAZ_00049017">
        <obo:RO_0001025 rdf:resource="http://purl.obolibrary.org/obo/GAZ_00012780"/>
        <obo:IAO_0000115>An island in the Solomon Islands; it is located in Choiseul Province.</obo:IAO_0000115>
        <oboInOwl:hasOBONamespace>GAZ</oboInOwl:hasOBONamespace>
        <oboInOwl:id>GAZ:00049017</oboInOwl:id>
        <rdfs:label>Vaghena Island</rdfs:label>
    </owl:NamedIndividual>
    


    <!-- http://purl.obolibrary.org/obo/GAZ_00049018 -->

    <owl:NamedIndividual rdf:about="http://purl.obolibrary.org/obo/GAZ_00049018">
        <obo:RO_0001025 rdf:resource="http://purl.obolibrary.org/obo/GAZ_00009558"/>
        <obo:IAO_0000115>A large island at the southern tip of the larger island of Malaita in the eastern part of the Solomon Islands.</obo:IAO_0000115>
        <oboInOwl:hasOBONamespace>GAZ</oboInOwl:hasOBONamespace>
        <oboInOwl:id>GAZ:00049018</oboInOwl:id>
        <rdfs:label>South Malaita Island</rdfs:label>
    </owl:NamedIndividual>
    


    <!-- http://purl.obolibrary.org/obo/GAZ_00051763 -->

    <owl:NamedIndividual rdf:about="http://purl.obolibrary.org/obo/GAZ_00051763">
        <obo:RO_0001025 rdf:resource="http://purl.obolibrary.org/obo/GAZ_00009133"/>
        <obo:IAO_0000115>A complex reef and lagoon system extending for 100 km from the northern end of New Georgia southeast along the northeastern coast of that island and around the north end of Vangunu Island to Nggatokae Island in the extreme east. The lagoon is bounded to the north and east by a string of narrow barrier islands which follow the entire coastline from the north end of New Georgia island southeast to Nggatokae. It encloses an area of 700 km2 within which there are over 300 small islands of varied geomorphology: sand cays, mangrove islets, raised reef islands and small islands of volcanic origin.</obo:IAO_0000115>
        <oboInOwl:hasOBONamespace>GAZ</oboInOwl:hasOBONamespace>
        <oboInOwl:id>GAZ:00051763</oboInOwl:id>
        <rdfs:label>Marovo Lagoon</rdfs:label>
    </owl:NamedIndividual>
    


    <!-- http://purl.obolibrary.org/obo/GAZ_00053799 -->

    <owl:NamedIndividual rdf:about="http://purl.obolibrary.org/obo/GAZ_00053799">
        <obo:RO_0001025 rdf:resource="http://purl.obolibrary.org/obo/GAZ_00007206"/>
        <obo:IAO_0000115>A brackish lake.</obo:IAO_0000115>
        <oboInOwl:hasOBONamespace>GAZ</oboInOwl:hasOBONamespace>
        <oboInOwl:id>GAZ:00053799</oboInOwl:id>
        <rdfs:label>Lake Te Nggano</rdfs:label>
    </owl:NamedIndividual>
    


    <!-- http://purl.obolibrary.org/obo/GAZ_00053955 -->

    <owl:NamedIndividual rdf:about="http://purl.obolibrary.org/obo/GAZ_00053955">
        <obo:RO_0001025 rdf:resource="http://purl.obolibrary.org/obo/GAZ_00016903"/>
        <obo:IAO_0000115>A lava dome located within a well-preserved crater.</obo:IAO_0000115>
        <oboInOwl:hasOBONamespace>GAZ</oboInOwl:hasOBONamespace>
        <oboInOwl:id>GAZ:00053955</oboInOwl:id>
        <rdfs:label>Nonda Volcano</rdfs:label>
    </owl:NamedIndividual>
    


    <!-- http://purl.obolibrary.org/obo/GAZ_00053956 -->

    <owl:NamedIndividual rdf:about="http://purl.obolibrary.org/obo/GAZ_00053956">
        <obo:RO_0001025 rdf:resource="http://purl.obolibrary.org/obo/GAZ_00016905"/>
        <obo:IAO_0000115>A stratovolcano.</obo:IAO_0000115>
        <oboInOwl:hasOBONamespace>GAZ</oboInOwl:hasOBONamespace>
        <oboInOwl:id>GAZ:00053956</oboInOwl:id>
        <rdfs:label>Mount Patukio</rdfs:label>
    </owl:NamedIndividual>
    


    <!-- http://purl.obolibrary.org/obo/GAZ_00053957 -->

    <owl:NamedIndividual rdf:about="http://purl.obolibrary.org/obo/GAZ_00053957">
        <obo:RO_0001025 rdf:resource="http://purl.obolibrary.org/obo/GAZ_00255949"/>
        <obo:IAO_0000115>A hot crater lake.</obo:IAO_0000115>
        <oboInOwl:hasOBONamespace>GAZ</oboInOwl:hasOBONamespace>
        <oboInOwl:id>GAZ:00053957</oboInOwl:id>
        <rdfs:label>Lake Ove</rdfs:label>
    </owl:NamedIndividual>
    


    <!-- http://purl.obolibrary.org/obo/GAZ_00053958 -->

    <owl:NamedIndividual rdf:about="http://purl.obolibrary.org/obo/GAZ_00053958">
        <obo:RO_0001025 rdf:resource="http://purl.obolibrary.org/obo/GAZ_00005275"/>
        <obo:IAO_0000115>An active dacitic submarine volcano SW of Rendova Island (Taylor, 1987). Kana Keoki Seamount, located along the Ghizo Ridge south of the convergent margin between the Indo-Australian and Pacific plates, rises to within about 700 m of the surface from a depth of 3700 m and is surrounded by a volcaniclastic apron.</obo:IAO_0000115>
        <oboInOwl:hasOBONamespace>GAZ</oboInOwl:hasOBONamespace>
        <oboInOwl:id>GAZ:00053958</oboInOwl:id>
        <rdfs:label>Kana Keoki Seamount</rdfs:label>
    </owl:NamedIndividual>
    


    <!-- http://purl.obolibrary.org/obo/GAZ_00053959 -->

    <owl:NamedIndividual rdf:about="http://purl.obolibrary.org/obo/GAZ_00053959">
        <obo:RO_0001025 rdf:resource="http://purl.obolibrary.org/obo/GAZ_00005275"/>
        <obo:IAO_0000115>A young submarine volcano SE of Kana Keoki seamount. The volcano was constructed over the eastern end of the inactive Woodlark spreading center, south of the convergent boundary between the Indo-Australian and Pacific plates. Coleman Seamount is undissected and probably even more recently active than Kana Keoki Seamount.</obo:IAO_0000115>
        <oboInOwl:hasOBONamespace>GAZ</oboInOwl:hasOBONamespace>
        <oboInOwl:id>GAZ:00053959</oboInOwl:id>
        <rdfs:label>Coleman Seamount</rdfs:label>
    </owl:NamedIndividual>
    


    <!-- http://purl.obolibrary.org/obo/GAZ_00053960 -->

    <owl:NamedIndividual rdf:about="http://purl.obolibrary.org/obo/GAZ_00053960">
        <obo:RO_0001025 rdf:resource="http://purl.obolibrary.org/obo/GAZ_00012781"/>
        <obo:IAO_0000115>A seamount that occupies an isolated position in the Solomon Islands far from major aircraft and shipping lanes. Kavachi is located south of Vangunu Island only about 30 km north of the site of subduction of the Indo-Australian plate beneath the Pacific plate. The shallow submarine basaltic-to-andesitic volcano has produced ephemeral islands up to 1 km long many times since its first recorded eruption during 1939.</obo:IAO_0000115>
        <oboInOwl:hasOBONamespace>GAZ</oboInOwl:hasOBONamespace>
        <oboInOwl:id>GAZ:00053960</oboInOwl:id>
        <rdfs:label>Kavachi Seamount</rdfs:label>
    </owl:NamedIndividual>
    


    <!-- http://purl.obolibrary.org/obo/GAZ_00053961 -->

    <owl:NamedIndividual rdf:about="http://purl.obolibrary.org/obo/GAZ_00053961">
        <obo:RO_0001025 rdf:resource="http://purl.obolibrary.org/obo/GAZ_00005276"/>
        <obo:IAO_0000115>A volcanic field comprising a group of steeply dissected cones, cover a large area of NW Guadalcanal Island (Hackman, 1980). Mount Roundhead is a small, but well-preserved volcano. Local traditions mention an historical eruption, but this could refer to an eruption from Savo volcano.</obo:IAO_0000115>
        <oboInOwl:hasOBONamespace>GAZ</oboInOwl:hasOBONamespace>
        <oboInOwl:id>GAZ:00053961</oboInOwl:id>
        <rdfs:label>Gallego Volcanic Field</rdfs:label>
    </owl:NamedIndividual>
    


    <!-- http://purl.obolibrary.org/obo/GAZ_00053962 -->

    <owl:NamedIndividual rdf:about="http://purl.obolibrary.org/obo/GAZ_00053962">
        <obo:RO_0001025 rdf:resource="http://purl.obolibrary.org/obo/GAZ_00053961"/>
        <obo:IAO_0000115>A volcano.</obo:IAO_0000115>
        <oboInOwl:hasOBONamespace>GAZ</oboInOwl:hasOBONamespace>
        <oboInOwl:id>GAZ:00053962</oboInOwl:id>
        <rdfs:label>Mount Roundhead</rdfs:label>
    </owl:NamedIndividual>
    


    <!-- http://purl.obolibrary.org/obo/GAZ_00147119 -->

    <owl:NamedIndividual rdf:about="http://purl.obolibrary.org/obo/GAZ_00147119">
        <rdf:type rdf:resource="http://purl.obolibrary.org/obo/ENVO_00000305"/>
        <obo:RO_0001025 rdf:resource="http://purl.obolibrary.org/obo/GAZ_00005276"/>
        <obo:IAO_0000115>A headland on the northern coast of Guadalcanal.</obo:IAO_0000115>
        <oboInOwl:hasOBONamespace>GAZ</oboInOwl:hasOBONamespace>
        <oboInOwl:id>GAZ:00147119</oboInOwl:id>
        <rdfs:label>Lunga Point</rdfs:label>
    </owl:NamedIndividual>
    


    <!-- http://purl.obolibrary.org/obo/GAZ_00147120 -->

    <owl:NamedIndividual rdf:about="http://purl.obolibrary.org/obo/GAZ_00147120">
        <rdf:type rdf:resource="http://purl.obolibrary.org/obo/ENVO_00000305"/>
        <obo:RO_0001025 rdf:resource="http://purl.obolibrary.org/obo/GAZ_00005276"/>
        <obo:IAO_0000115>A headland on the north shore of Guadalcanal, Solomon Islands.</obo:IAO_0000115>
        <oboInOwl:hasOBONamespace>GAZ</oboInOwl:hasOBONamespace>
        <oboInOwl:id>GAZ:00147120</oboInOwl:id>
        <rdfs:label>Tassafaronga Point</rdfs:label>
    </owl:NamedIndividual>
    


    <!-- http://purl.obolibrary.org/obo/GAZ_00147121 -->

    <owl:NamedIndividual rdf:about="http://purl.obolibrary.org/obo/GAZ_00147121">
        <obo:RO_0001025 rdf:resource="http://purl.obolibrary.org/obo/GAZ_00005276"/>
        <obo:IAO_0000115>The northernmost point on Guadalcanal, Solomon Islands.</obo:IAO_0000115>
        <oboInOwl:hasOBONamespace>GAZ</oboInOwl:hasOBONamespace>
        <oboInOwl:id>GAZ:00147121</oboInOwl:id>
        <rdfs:label>Cape Esperance</rdfs:label>
    </owl:NamedIndividual>
    


    <!-- http://purl.obolibrary.org/obo/GAZ_00148032 -->

    <owl:NamedIndividual rdf:about="http://purl.obolibrary.org/obo/GAZ_00148032">
        <obo:RO_0001025 rdf:resource="http://purl.obolibrary.org/obo/GAZ_00012781"/>
        <obo:IAO_0000115>A waterway in the Western Province of the Solomon Islands. It lies between the islands of Kolombangara to the north, and Arundel Island (Kohinggo) to the south. It connects Vella Gulf to the west with Kula Gulf to the east.</obo:IAO_0000115>
        <oboInOwl:hasOBONamespace>GAZ</oboInOwl:hasOBONamespace>
        <oboInOwl:id>GAZ:00148032</oboInOwl:id>
        <rdfs:label>Blackett Strait</rdfs:label>
    </owl:NamedIndividual>
    


    <!-- http://purl.obolibrary.org/obo/GAZ_00148034 -->

    <owl:NamedIndividual rdf:about="http://purl.obolibrary.org/obo/GAZ_00148034">
        <obo:RO_0001025 rdf:resource="http://purl.obolibrary.org/obo/GAZ_00009135"/>
        <obo:IAO_0000115>One of the Russell Islands.</obo:IAO_0000115>
        <oboInOwl:hasOBONamespace>GAZ</oboInOwl:hasOBONamespace>
        <oboInOwl:id>GAZ:00148034</oboInOwl:id>
        <rdfs:label>Mbanika Island</rdfs:label>
    </owl:NamedIndividual>
    


    <!-- http://purl.obolibrary.org/obo/GAZ_00148035 -->

    <owl:NamedIndividual rdf:about="http://purl.obolibrary.org/obo/GAZ_00148035">
        <obo:RO_0001025 rdf:resource="http://purl.obolibrary.org/obo/GAZ_00012780"/>
        <obo:IAO_0000115>An island in the Solomon Islands; it is located in Choiseul Province.</obo:IAO_0000115>
        <oboInOwl:hasOBONamespace>GAZ</oboInOwl:hasOBONamespace>
        <oboInOwl:id>GAZ:00148035</oboInOwl:id>
        <rdfs:label>Nuatambu Island</rdfs:label>
    </owl:NamedIndividual>
    


    <!-- http://purl.obolibrary.org/obo/GAZ_00148036 -->

    <owl:NamedIndividual rdf:about="http://purl.obolibrary.org/obo/GAZ_00148036">
        <obo:RO_0001025 rdf:resource="http://purl.obolibrary.org/obo/GAZ_00012783"/>
        <obo:IAO_0000115>An island in the Solomon Islands; it is located in the Central Province.</obo:IAO_0000115>
        <oboInOwl:hasOBONamespace>GAZ</oboInOwl:hasOBONamespace>
        <oboInOwl:id>GAZ:00148036</oboInOwl:id>
        <rdfs:label>Aeaun Island</rdfs:label>
    </owl:NamedIndividual>
    


    <!-- http://purl.obolibrary.org/obo/GAZ_00148042 -->

    <owl:NamedIndividual rdf:about="http://purl.obolibrary.org/obo/GAZ_00148042">
        <rdf:type rdf:resource="http://purl.obolibrary.org/obo/ENVO_00000029"/>
        <obo:RO_0001025 rdf:resource="http://purl.obolibrary.org/obo/GAZ_00009558"/>
        <obo:IAO_0000115>A narrow passage which separates the two islands of Malaita Province in the Solomon Islands, the larger Malaita and the smaller South Malaita Island.</obo:IAO_0000115>
        <oboInOwl:hasOBONamespace>GAZ</oboInOwl:hasOBONamespace>
        <oboInOwl:id>GAZ:00148042</oboInOwl:id>
        <rdfs:label>Maramasike Passage</rdfs:label>
    </owl:NamedIndividual>
    


    <!-- http://purl.obolibrary.org/obo/GAZ_00255724 -->

    <owl:NamedIndividual rdf:about="http://purl.obolibrary.org/obo/GAZ_00255724">
        <obo:RO_0001025 rdf:resource="http://purl.obolibrary.org/obo/GAZ_00016910"/>
        <obo:IAO_0000115>An island.</obo:IAO_0000115>
        <oboInOwl:hasOBONamespace>GAZ</oboInOwl:hasOBONamespace>
        <oboInOwl:id>GAZ:00255724</oboInOwl:id>
        <rdfs:label>Olevugha Island</rdfs:label>
    </owl:NamedIndividual>
    


    <!-- http://purl.obolibrary.org/obo/GAZ_00255725 -->

    <owl:NamedIndividual rdf:about="http://purl.obolibrary.org/obo/GAZ_00255725">
        <obo:RO_0001025 rdf:resource="http://purl.obolibrary.org/obo/GAZ_00016910"/>
        <obo:IAO_0000115>An island.</obo:IAO_0000115>
        <oboInOwl:hasOBONamespace>GAZ</oboInOwl:hasOBONamespace>
        <oboInOwl:id>GAZ:00255725</oboInOwl:id>
        <rdfs:label>Vatilau Island</rdfs:label>
    </owl:NamedIndividual>
    


    <!-- http://purl.obolibrary.org/obo/GAZ_00255726 -->

    <owl:NamedIndividual rdf:about="http://purl.obolibrary.org/obo/GAZ_00255726">
        <rdf:type rdf:resource="http://purl.obolibrary.org/obo/ENVO_00000856"/>
        <obo:RO_0001025 rdf:resource="http://purl.obolibrary.org/obo/GAZ_00148034"/>
        <obo:IAO_0000115>A populated place. A town on Mbanika Island in the Russell Islands, in the Central Province of the Solomon Islands.</obo:IAO_0000115>
        <oboInOwl:hasOBONamespace>GAZ</oboInOwl:hasOBONamespace>
        <oboInOwl:id>GAZ:00255726</oboInOwl:id>
        <rdfs:label>Yandina</rdfs:label>
    </owl:NamedIndividual>
    


    <!-- http://purl.obolibrary.org/obo/GAZ_00255727 -->

    <owl:NamedIndividual rdf:about="http://purl.obolibrary.org/obo/GAZ_00255727">
        <obo:RO_0001025 rdf:resource="http://purl.obolibrary.org/obo/GAZ_00009138"/>
        <obo:IAO_0000115>A populated place.</obo:IAO_0000115>
        <oboInOwl:hasOBONamespace>GAZ</oboInOwl:hasOBONamespace>
        <oboInOwl:id>GAZ:00255727</oboInOwl:id>
        <rdfs:label>Polo</rdfs:label>
    </owl:NamedIndividual>
    


    <!-- http://purl.obolibrary.org/obo/GAZ_00255728 -->

    <owl:NamedIndividual rdf:about="http://purl.obolibrary.org/obo/GAZ_00255728">
        <obo:RO_0001025 rdf:resource="http://purl.obolibrary.org/obo/GAZ_00009138"/>
        <obo:IAO_0000115>A populated place.</obo:IAO_0000115>
        <oboInOwl:hasOBONamespace>GAZ</oboInOwl:hasOBONamespace>
        <oboInOwl:id>GAZ:00255728</oboInOwl:id>
        <rdfs:label>Pangooe</rdfs:label>
    </owl:NamedIndividual>
    


    <!-- http://purl.obolibrary.org/obo/GAZ_00255729 -->

    <owl:NamedIndividual rdf:about="http://purl.obolibrary.org/obo/GAZ_00255729">
        <rdf:type rdf:resource="http://purl.obolibrary.org/obo/ENVO_00000222"/>
        <obo:RO_0001025 rdf:resource="http://purl.obolibrary.org/obo/GAZ_00012780"/>
        <obo:IAO_0000115>A small island located amongst the Solomon Islands. A volcanic island that lies between the islands of Fauro (30 km to the southwest) and Choiseu about 100 km to the northeast).</obo:IAO_0000115>
        <oboInOwl:hasOBONamespace>GAZ</oboInOwl:hasOBONamespace>
        <oboInOwl:id>GAZ:00255729</oboInOwl:id>
        <rdfs:label>Cyprian Bridge Island</rdfs:label>
    </owl:NamedIndividual>
    


    <!-- http://purl.obolibrary.org/obo/GAZ_00255730 -->

    <owl:NamedIndividual rdf:about="http://purl.obolibrary.org/obo/GAZ_00255730">
        <obo:RO_0001025 rdf:resource="http://purl.obolibrary.org/obo/GAZ_00009138"/>
        <obo:IAO_0000115>A populated place.</obo:IAO_0000115>
        <oboInOwl:hasOBONamespace>GAZ</oboInOwl:hasOBONamespace>
        <oboInOwl:id>GAZ:00255730</oboInOwl:id>
        <rdfs:label>Posarae</rdfs:label>
    </owl:NamedIndividual>
    


    <!-- http://purl.obolibrary.org/obo/GAZ_00255731 -->

    <owl:NamedIndividual rdf:about="http://purl.obolibrary.org/obo/GAZ_00255731">
        <obo:RO_0001025 rdf:resource="http://purl.obolibrary.org/obo/GAZ_00009138"/>
        <obo:IAO_0000115>A populated place.</obo:IAO_0000115>
        <oboInOwl:hasOBONamespace>GAZ</oboInOwl:hasOBONamespace>
        <oboInOwl:id>GAZ:00255731</oboInOwl:id>
        <rdfs:label>Poroporo</rdfs:label>
    </owl:NamedIndividual>
    


    <!-- http://purl.obolibrary.org/obo/GAZ_00255732 -->

    <owl:NamedIndividual rdf:about="http://purl.obolibrary.org/obo/GAZ_00255732">
        <obo:RO_0001025 rdf:resource="http://purl.obolibrary.org/obo/GAZ_00009138"/>
        <obo:IAO_0000115>A populated place.</obo:IAO_0000115>
        <oboInOwl:hasOBONamespace>GAZ</oboInOwl:hasOBONamespace>
        <oboInOwl:id>GAZ:00255732</oboInOwl:id>
        <rdfs:label>Nukiki</rdfs:label>
    </owl:NamedIndividual>
    


    <!-- http://purl.obolibrary.org/obo/GAZ_00255733 -->

    <owl:NamedIndividual rdf:about="http://purl.obolibrary.org/obo/GAZ_00255733">
        <obo:RO_0001025 rdf:resource="http://purl.obolibrary.org/obo/GAZ_00009138"/>
        <obo:IAO_0000115>A populated place.</obo:IAO_0000115>
        <oboInOwl:hasOBONamespace>GAZ</oboInOwl:hasOBONamespace>
        <oboInOwl:id>GAZ:00255733</oboInOwl:id>
        <rdfs:label>Zavare</rdfs:label>
    </owl:NamedIndividual>
    


    <!-- http://purl.obolibrary.org/obo/GAZ_00255734 -->

    <owl:NamedIndividual rdf:about="http://purl.obolibrary.org/obo/GAZ_00255734">
        <obo:RO_0001025 rdf:resource="http://purl.obolibrary.org/obo/GAZ_00009138"/>
        <obo:IAO_0000115>A populated place.</obo:IAO_0000115>
        <oboInOwl:hasOBONamespace>GAZ</oboInOwl:hasOBONamespace>
        <oboInOwl:id>GAZ:00255734</oboInOwl:id>
        <rdfs:label>Sasamungga</rdfs:label>
    </owl:NamedIndividual>
    


    <!-- http://purl.obolibrary.org/obo/GAZ_00255735 -->

    <owl:NamedIndividual rdf:about="http://purl.obolibrary.org/obo/GAZ_00255735">
        <obo:RO_0001025 rdf:resource="http://purl.obolibrary.org/obo/GAZ_00255926"/>
        <obo:IAO_0000115>A populated place. The capital of the Solomon Islands and of Guadalcanal Province.</obo:IAO_0000115>
        <oboInOwl:hasOBONamespace>GAZ</oboInOwl:hasOBONamespace>
        <oboInOwl:id>GAZ:00255735</oboInOwl:id>
        <rdfs:label>Honiara</rdfs:label>
    </owl:NamedIndividual>
    


    <!-- http://purl.obolibrary.org/obo/GAZ_00255736 -->

    <owl:NamedIndividual rdf:about="http://purl.obolibrary.org/obo/GAZ_00255736">
        <obo:RO_0001025 rdf:resource="http://purl.obolibrary.org/obo/GAZ_00005276"/>
        <obo:IAO_0000115>A populated place.</obo:IAO_0000115>
        <oboInOwl:hasOBONamespace>GAZ</oboInOwl:hasOBONamespace>
        <oboInOwl:id>GAZ:00255736</oboInOwl:id>
        <rdfs:label>Tutumu</rdfs:label>
    </owl:NamedIndividual>
    


    <!-- http://purl.obolibrary.org/obo/GAZ_00255737 -->

    <owl:NamedIndividual rdf:about="http://purl.obolibrary.org/obo/GAZ_00255737">
        <obo:RO_0001025 rdf:resource="http://purl.obolibrary.org/obo/GAZ_00005276"/>
        <obo:IAO_0000115>A populated place.</obo:IAO_0000115>
        <oboInOwl:hasOBONamespace>GAZ</oboInOwl:hasOBONamespace>
        <oboInOwl:id>GAZ:00255737</oboInOwl:id>
        <rdfs:label>Nduindui</rdfs:label>
    </owl:NamedIndividual>
    


    <!-- http://purl.obolibrary.org/obo/GAZ_00255738 -->

    <owl:NamedIndividual rdf:about="http://purl.obolibrary.org/obo/GAZ_00255738">
        <obo:RO_0001025 rdf:resource="http://purl.obolibrary.org/obo/GAZ_00005276"/>
        <obo:IAO_0000115>A populated place.</obo:IAO_0000115>
        <oboInOwl:hasOBONamespace>GAZ</oboInOwl:hasOBONamespace>
        <oboInOwl:id>GAZ:00255738</oboInOwl:id>
        <rdfs:label>Avu Avu</rdfs:label>
    </owl:NamedIndividual>
    


    <!-- http://purl.obolibrary.org/obo/GAZ_00255739 -->

    <owl:NamedIndividual rdf:about="http://purl.obolibrary.org/obo/GAZ_00255739">
        <obo:RO_0001025 rdf:resource="http://purl.obolibrary.org/obo/GAZ_00005276"/>
        <obo:IAO_0000115>A populated place.</obo:IAO_0000115>
        <oboInOwl:hasOBONamespace>GAZ</oboInOwl:hasOBONamespace>
        <oboInOwl:id>GAZ:00255739</oboInOwl:id>
        <rdfs:label>Paruru</rdfs:label>
    </owl:NamedIndividual>
    


    <!-- http://purl.obolibrary.org/obo/GAZ_00255740 -->

    <owl:NamedIndividual rdf:about="http://purl.obolibrary.org/obo/GAZ_00255740">
        <obo:RO_0001025 rdf:resource="http://purl.obolibrary.org/obo/GAZ_00009555"/>
        <obo:IAO_0000115>An island in the Solomon Islands; it is located in Guadalcanal Province.</obo:IAO_0000115>
        <oboInOwl:hasOBONamespace>GAZ</oboInOwl:hasOBONamespace>
        <oboInOwl:id>GAZ:00255740</oboInOwl:id>
        <rdfs:label>Korasahalu Island</rdfs:label>
    </owl:NamedIndividual>
    


    <!-- http://purl.obolibrary.org/obo/GAZ_00255741 -->

    <owl:NamedIndividual rdf:about="http://purl.obolibrary.org/obo/GAZ_00255741">
        <obo:RO_0001025 rdf:resource="http://purl.obolibrary.org/obo/GAZ_00009555"/>
        <obo:IAO_0000115>An island in the Solomon Islands; it is located in Guadalcanal Province.</obo:IAO_0000115>
        <oboInOwl:hasOBONamespace>GAZ</oboInOwl:hasOBONamespace>
        <oboInOwl:id>GAZ:00255741</oboInOwl:id>
        <rdfs:label>Nughu Island</rdfs:label>
    </owl:NamedIndividual>
    


    <!-- http://purl.obolibrary.org/obo/GAZ_00255742 -->

    <owl:NamedIndividual rdf:about="http://purl.obolibrary.org/obo/GAZ_00255742">
        <obo:RO_0001025 rdf:resource="http://purl.obolibrary.org/obo/GAZ_00009555"/>
        <obo:IAO_0000115>An island in the Solomon Islands; it is located in Guadalcanal Province.</obo:IAO_0000115>
        <oboInOwl:hasOBONamespace>GAZ</oboInOwl:hasOBONamespace>
        <oboInOwl:id>GAZ:00255742</oboInOwl:id>
        <rdfs:label>Tavanipupu Island</rdfs:label>
    </owl:NamedIndividual>
    


    <!-- http://purl.obolibrary.org/obo/GAZ_00255743 -->

    <owl:NamedIndividual rdf:about="http://purl.obolibrary.org/obo/GAZ_00255743">
        <obo:RO_0001025 rdf:resource="http://purl.obolibrary.org/obo/GAZ_00009555"/>
        <obo:IAO_0000115>An island in the Solomon Islands; it is located in Guadalcanal Province.</obo:IAO_0000115>
        <oboInOwl:hasOBONamespace>GAZ</oboInOwl:hasOBONamespace>
        <oboInOwl:id>GAZ:00255743</oboInOwl:id>
        <rdfs:label>Vulelua Island</rdfs:label>
    </owl:NamedIndividual>
    


    <!-- http://purl.obolibrary.org/obo/GAZ_00255745 -->

    <owl:NamedIndividual rdf:about="http://purl.obolibrary.org/obo/GAZ_00255745">
        <obo:RO_0001025 rdf:resource="http://purl.obolibrary.org/obo/GAZ_00009556"/>
        <obo:IAO_0000115>A chain of three large coral atolls in the Coral Sea. They are located about 50 km south of Rennell Island, separated from it by Rennel Trough. The chain stretches over a length of 114 km and its average width is 18 km. Administratively the Indispensable Reef belongs to the Rennell and Bellona Province of the Solomon Islands.</obo:IAO_0000115>
        <oboInOwl:hasOBONamespace>GAZ</oboInOwl:hasOBONamespace>
        <oboInOwl:id>GAZ:00255745</oboInOwl:id>
        <rdfs:label>Indispensable Reefs</rdfs:label>
    </owl:NamedIndividual>
    


    <!-- http://purl.obolibrary.org/obo/GAZ_00255746 -->

    <owl:NamedIndividual rdf:about="http://purl.obolibrary.org/obo/GAZ_00255746">
        <obo:RO_0001025 rdf:resource="http://purl.obolibrary.org/obo/GAZ_00255745"/>
        <obo:IAO_0000115>A coral reef.</obo:IAO_0000115>
        <oboInOwl:hasOBONamespace>GAZ</oboInOwl:hasOBONamespace>
        <oboInOwl:id>GAZ:00255746</oboInOwl:id>
        <rdfs:label>Indispensable Reef North</rdfs:label>
    </owl:NamedIndividual>
    


    <!-- http://purl.obolibrary.org/obo/GAZ_00255747 -->

    <owl:NamedIndividual rdf:about="http://purl.obolibrary.org/obo/GAZ_00255747">
        <rdf:type rdf:resource="http://purl.obolibrary.org/obo/ENVO_00000856"/>
        <obo:RO_0001025 rdf:resource="http://purl.obolibrary.org/obo/GAZ_00009136"/>
        <obo:IAO_0000115>A populated place. A town located on Santa Isabel Island.</obo:IAO_0000115>
        <oboInOwl:hasOBONamespace>GAZ</oboInOwl:hasOBONamespace>
        <oboInOwl:id>GAZ:00255747</oboInOwl:id>
        <rdfs:label>Buala</rdfs:label>
    </owl:NamedIndividual>
    


    <!-- http://purl.obolibrary.org/obo/GAZ_00255748 -->

    <owl:NamedIndividual rdf:about="http://purl.obolibrary.org/obo/GAZ_00255748">
        <obo:RO_0001025 rdf:resource="http://purl.obolibrary.org/obo/GAZ_00009136"/>
        <obo:IAO_0000115>A populated place.</obo:IAO_0000115>
        <oboInOwl:hasOBONamespace>GAZ</oboInOwl:hasOBONamespace>
        <oboInOwl:id>GAZ:00255748</oboInOwl:id>
        <rdfs:label>Kia</rdfs:label>
    </owl:NamedIndividual>
    


    <!-- http://purl.obolibrary.org/obo/GAZ_00255749 -->

    <owl:NamedIndividual rdf:about="http://purl.obolibrary.org/obo/GAZ_00255749">
        <obo:RO_0001025 rdf:resource="http://purl.obolibrary.org/obo/GAZ_00009136"/>
        <obo:IAO_0000115>A populated place.</obo:IAO_0000115>
        <oboInOwl:hasOBONamespace>GAZ</oboInOwl:hasOBONamespace>
        <oboInOwl:id>GAZ:00255749</oboInOwl:id>
        <rdfs:label>Baolo</rdfs:label>
    </owl:NamedIndividual>
    


    <!-- http://purl.obolibrary.org/obo/GAZ_00255750 -->

    <owl:NamedIndividual rdf:about="http://purl.obolibrary.org/obo/GAZ_00255750">
        <obo:RO_0001025 rdf:resource="http://purl.obolibrary.org/obo/GAZ_00009136"/>
        <obo:IAO_0000115>A populated place.</obo:IAO_0000115>
        <oboInOwl:hasOBONamespace>GAZ</oboInOwl:hasOBONamespace>
        <oboInOwl:id>GAZ:00255750</oboInOwl:id>
        <rdfs:label>Bolitei</rdfs:label>
    </owl:NamedIndividual>
    


    <!-- http://purl.obolibrary.org/obo/GAZ_00255751 -->

    <owl:NamedIndividual rdf:about="http://purl.obolibrary.org/obo/GAZ_00255751">
        <obo:RO_0001025 rdf:resource="http://purl.obolibrary.org/obo/GAZ_00009136"/>
        <obo:IAO_0000115>A populated place.</obo:IAO_0000115>
        <oboInOwl:hasOBONamespace>GAZ</oboInOwl:hasOBONamespace>
        <oboInOwl:id>GAZ:00255751</oboInOwl:id>
        <rdfs:label>Ghoveo</rdfs:label>
    </owl:NamedIndividual>
    


    <!-- http://purl.obolibrary.org/obo/GAZ_00255752 -->

    <owl:NamedIndividual rdf:about="http://purl.obolibrary.org/obo/GAZ_00255752">
        <obo:RO_0001025 rdf:resource="http://purl.obolibrary.org/obo/GAZ_00009136"/>
        <obo:IAO_0000115>A populated place.</obo:IAO_0000115>
        <oboInOwl:hasOBONamespace>GAZ</oboInOwl:hasOBONamespace>
        <oboInOwl:id>GAZ:00255752</oboInOwl:id>
        <rdfs:label>Kmagha</rdfs:label>
    </owl:NamedIndividual>
    


    <!-- http://purl.obolibrary.org/obo/GAZ_00255753 -->

    <owl:NamedIndividual rdf:about="http://purl.obolibrary.org/obo/GAZ_00255753">
        <obo:RO_0001025 rdf:resource="http://purl.obolibrary.org/obo/GAZ_00009136"/>
        <obo:IAO_0000115>A populated place.</obo:IAO_0000115>
        <oboInOwl:hasOBONamespace>GAZ</oboInOwl:hasOBONamespace>
        <oboInOwl:id>GAZ:00255753</oboInOwl:id>
        <rdfs:label>Sau&apos;a</rdfs:label>
    </owl:NamedIndividual>
    


    <!-- http://purl.obolibrary.org/obo/GAZ_00255754 -->

    <owl:NamedIndividual rdf:about="http://purl.obolibrary.org/obo/GAZ_00255754">
        <obo:RO_0001025 rdf:resource="http://purl.obolibrary.org/obo/GAZ_00009136"/>
        <obo:IAO_0000115>A populated place.</obo:IAO_0000115>
        <oboInOwl:hasOBONamespace>GAZ</oboInOwl:hasOBONamespace>
        <oboInOwl:id>GAZ:00255754</oboInOwl:id>
        <rdfs:label>Sidu</rdfs:label>
    </owl:NamedIndividual>
    


    <!-- http://purl.obolibrary.org/obo/GAZ_00255755 -->

    <owl:NamedIndividual rdf:about="http://purl.obolibrary.org/obo/GAZ_00255755">
        <obo:RO_0001025 rdf:resource="http://purl.obolibrary.org/obo/GAZ_00009136"/>
        <obo:IAO_0000115>A populated place.</obo:IAO_0000115>
        <oboInOwl:hasOBONamespace>GAZ</oboInOwl:hasOBONamespace>
        <oboInOwl:id>GAZ:00255755</oboInOwl:id>
        <rdfs:label>Sepi</rdfs:label>
    </owl:NamedIndividual>
    


    <!-- http://purl.obolibrary.org/obo/GAZ_00255756 -->

    <owl:NamedIndividual rdf:about="http://purl.obolibrary.org/obo/GAZ_00255756">
        <obo:RO_0001025 rdf:resource="http://purl.obolibrary.org/obo/GAZ_00009136"/>
        <obo:IAO_0000115>A populated place.</obo:IAO_0000115>
        <oboInOwl:hasOBONamespace>GAZ</oboInOwl:hasOBONamespace>
        <oboInOwl:id>GAZ:00255756</oboInOwl:id>
        <rdfs:label>Tuaraghu</rdfs:label>
    </owl:NamedIndividual>
    


    <!-- http://purl.obolibrary.org/obo/GAZ_00255757 -->

    <owl:NamedIndividual rdf:about="http://purl.obolibrary.org/obo/GAZ_00255757">
        <obo:RO_0001025 rdf:resource="http://purl.obolibrary.org/obo/GAZ_00009136"/>
        <obo:IAO_0000115>A populated place.</obo:IAO_0000115>
        <oboInOwl:hasOBONamespace>GAZ</oboInOwl:hasOBONamespace>
        <oboInOwl:id>GAZ:00255757</oboInOwl:id>
        <rdfs:label>Dadale</rdfs:label>
    </owl:NamedIndividual>
    


    <!-- http://purl.obolibrary.org/obo/GAZ_00255758 -->

    <owl:NamedIndividual rdf:about="http://purl.obolibrary.org/obo/GAZ_00255758">
        <obo:RO_0001025 rdf:resource="http://purl.obolibrary.org/obo/GAZ_00009136"/>
        <obo:IAO_0000115>A populated place.</obo:IAO_0000115>
        <oboInOwl:hasOBONamespace>GAZ</oboInOwl:hasOBONamespace>
        <oboInOwl:id>GAZ:00255758</oboInOwl:id>
        <rdfs:label>Samasodu</rdfs:label>
    </owl:NamedIndividual>
    


    <!-- http://purl.obolibrary.org/obo/GAZ_00255759 -->

    <owl:NamedIndividual rdf:about="http://purl.obolibrary.org/obo/GAZ_00255759">
        <obo:RO_0001025 rdf:resource="http://purl.obolibrary.org/obo/GAZ_00009136"/>
        <obo:IAO_0000115>A populated place.</obo:IAO_0000115>
        <oboInOwl:hasOBONamespace>GAZ</oboInOwl:hasOBONamespace>
        <oboInOwl:id>GAZ:00255759</oboInOwl:id>
        <rdfs:label>Filuo</rdfs:label>
    </owl:NamedIndividual>
    


    <!-- http://purl.obolibrary.org/obo/GAZ_00255760 -->

    <owl:NamedIndividual rdf:about="http://purl.obolibrary.org/obo/GAZ_00255760">
        <obo:RO_0001025 rdf:resource="http://purl.obolibrary.org/obo/GAZ_00255929"/>
        <obo:IAO_0000115>An island in the Solomon Islands; it is located in Isabel Province. A reef.</obo:IAO_0000115>
        <oboInOwl:hasOBONamespace>GAZ</oboInOwl:hasOBONamespace>
        <oboInOwl:id>GAZ:00255760</oboInOwl:id>
        <rdfs:label>Sikopo Island</rdfs:label>
    </owl:NamedIndividual>
    


    <!-- http://purl.obolibrary.org/obo/GAZ_00255761 -->

    <owl:NamedIndividual rdf:about="http://purl.obolibrary.org/obo/GAZ_00255761">
        <obo:RO_0001025 rdf:resource="http://purl.obolibrary.org/obo/GAZ_00009136"/>
        <obo:IAO_0000115>A bay located on the south coast of Santa Isabel Island in the Solomon Islands, between San Jorge Island and Santa Isabelle.</obo:IAO_0000115>
        <oboInOwl:hasOBONamespace>GAZ</oboInOwl:hasOBONamespace>
        <oboInOwl:id>GAZ:00255761</oboInOwl:id>
        <rdfs:label>Thousand Ships Bay</rdfs:label>
    </owl:NamedIndividual>
    


    <!-- http://purl.obolibrary.org/obo/GAZ_00255762 -->

    <owl:NamedIndividual rdf:about="http://purl.obolibrary.org/obo/GAZ_00255762">
        <obo:RO_0001025 rdf:resource="http://purl.obolibrary.org/obo/GAZ_00012782"/>
        <obo:IAO_0000115>The channel between Choiseul Island and Santa Isabel Island.</obo:IAO_0000115>
        <oboInOwl:hasOBONamespace>GAZ</oboInOwl:hasOBONamespace>
        <oboInOwl:id>GAZ:00255762</oboInOwl:id>
        <rdfs:label>Manning Strait</rdfs:label>
    </owl:NamedIndividual>
    


    <!-- http://purl.obolibrary.org/obo/GAZ_00255763 -->

    <owl:NamedIndividual rdf:about="http://purl.obolibrary.org/obo/GAZ_00255763">
        <obo:RO_0001025 rdf:resource="http://purl.obolibrary.org/obo/GAZ_00255929"/>
        <obo:IAO_0000115>An island in the Solomon Islands; it is located in Isabel Province. A reef.</obo:IAO_0000115>
        <oboInOwl:hasOBONamespace>GAZ</oboInOwl:hasOBONamespace>
        <oboInOwl:id>GAZ:00255763</oboInOwl:id>
        <rdfs:label>Kerehikapa Island</rdfs:label>
    </owl:NamedIndividual>
    


    <!-- http://purl.obolibrary.org/obo/GAZ_00255764 -->

    <owl:NamedIndividual rdf:about="http://purl.obolibrary.org/obo/GAZ_00255764">
        <obo:RO_0001025 rdf:resource="http://purl.obolibrary.org/obo/GAZ_00255929"/>
        <obo:IAO_0000115>An island in the Solomon Islands; it is located in Isabel Province. A reef.</obo:IAO_0000115>
        <oboInOwl:hasOBONamespace>GAZ</oboInOwl:hasOBONamespace>
        <oboInOwl:id>GAZ:00255764</oboInOwl:id>
        <rdfs:label>Maleivona Island</rdfs:label>
    </owl:NamedIndividual>
    


    <!-- http://purl.obolibrary.org/obo/GAZ_00255765 -->

    <owl:NamedIndividual rdf:about="http://purl.obolibrary.org/obo/GAZ_00255765">
        <obo:RO_0001025 rdf:resource="http://purl.obolibrary.org/obo/GAZ_00012782"/>
        <obo:IAO_0000115>An island in the Solomon Islands; it is located in Isabel Province.</obo:IAO_0000115>
        <oboInOwl:hasOBONamespace>GAZ</oboInOwl:hasOBONamespace>
        <oboInOwl:id>GAZ:00255765</oboInOwl:id>
        <rdfs:label>Ramos Island</rdfs:label>
    </owl:NamedIndividual>
    


    <!-- http://purl.obolibrary.org/obo/GAZ_00255766 -->

    <owl:NamedIndividual rdf:about="http://purl.obolibrary.org/obo/GAZ_00255766">
        <obo:RO_0001025 rdf:resource="http://purl.obolibrary.org/obo/GAZ_00012782"/>
        <obo:IAO_0000115>An island.</obo:IAO_0000115>
        <oboInOwl:hasOBONamespace>GAZ</oboInOwl:hasOBONamespace>
        <oboInOwl:id>GAZ:00255766</oboInOwl:id>
        <rdfs:label>Mahige Island</rdfs:label>
    </owl:NamedIndividual>
    


    <!-- http://purl.obolibrary.org/obo/GAZ_00255767 -->

    <owl:NamedIndividual rdf:about="http://purl.obolibrary.org/obo/GAZ_00255767">
        <obo:RO_0001025 rdf:resource="http://purl.obolibrary.org/obo/GAZ_00012779"/>
        <obo:IAO_0000115>An island in the Solomon Islands province of Makira-Ulawa. It is situated 4 km north-west of Ugi Island.</obo:IAO_0000115>
        <oboInOwl:hasOBONamespace>GAZ</oboInOwl:hasOBONamespace>
        <oboInOwl:id>GAZ:00255767</oboInOwl:id>
        <rdfs:label>Pio Island</rdfs:label>
    </owl:NamedIndividual>
    


    <!-- http://purl.obolibrary.org/obo/GAZ_00255768 -->

    <owl:NamedIndividual rdf:about="http://purl.obolibrary.org/obo/GAZ_00255768">
        <obo:RO_0001025 rdf:resource="http://purl.obolibrary.org/obo/GAZ_00012779"/>
        <obo:IAO_0000115>An island in the Solomon Islands; it is located in Makira-Ulawa Province.</obo:IAO_0000115>
        <oboInOwl:hasOBONamespace>GAZ</oboInOwl:hasOBONamespace>
        <oboInOwl:id>GAZ:00255768</oboInOwl:id>
        <rdfs:label>Malaupaina Island</rdfs:label>
    </owl:NamedIndividual>
    


    <!-- http://purl.obolibrary.org/obo/GAZ_00255769 -->

    <owl:NamedIndividual rdf:about="http://purl.obolibrary.org/obo/GAZ_00255769">
        <obo:RO_0001025 rdf:resource="http://purl.obolibrary.org/obo/GAZ_00009134"/>
        <obo:IAO_0000115>A populated place.</obo:IAO_0000115>
        <oboInOwl:hasOBONamespace>GAZ</oboInOwl:hasOBONamespace>
        <oboInOwl:id>GAZ:00255769</oboInOwl:id>
        <rdfs:label>Ubana</rdfs:label>
    </owl:NamedIndividual>
    


    <!-- http://purl.obolibrary.org/obo/GAZ_00255770 -->

    <owl:NamedIndividual rdf:about="http://purl.obolibrary.org/obo/GAZ_00255770">
        <obo:RO_0001025 rdf:resource="http://purl.obolibrary.org/obo/GAZ_00009134"/>
        <obo:IAO_0000115>A populated place.</obo:IAO_0000115>
        <oboInOwl:hasOBONamespace>GAZ</oboInOwl:hasOBONamespace>
        <oboInOwl:id>GAZ:00255770</oboInOwl:id>
        <rdfs:label>Hada</rdfs:label>
    </owl:NamedIndividual>
    


    <!-- http://purl.obolibrary.org/obo/GAZ_00255771 -->

    <owl:NamedIndividual rdf:about="http://purl.obolibrary.org/obo/GAZ_00255771">
        <obo:RO_0001025 rdf:resource="http://purl.obolibrary.org/obo/GAZ_00009134"/>
        <obo:IAO_0000115>A populated place.</obo:IAO_0000115>
        <oboInOwl:hasOBONamespace>GAZ</oboInOwl:hasOBONamespace>
        <oboInOwl:id>GAZ:00255771</oboInOwl:id>
        <rdfs:label>Suruaharau</rdfs:label>
    </owl:NamedIndividual>
    


    <!-- http://purl.obolibrary.org/obo/GAZ_00255772 -->

    <owl:NamedIndividual rdf:about="http://purl.obolibrary.org/obo/GAZ_00255772">
        <obo:RO_0001025 rdf:resource="http://purl.obolibrary.org/obo/GAZ_00009134"/>
        <obo:IAO_0000115>A populated place.</obo:IAO_0000115>
        <oboInOwl:hasOBONamespace>GAZ</oboInOwl:hasOBONamespace>
        <oboInOwl:id>GAZ:00255772</oboInOwl:id>
        <rdfs:label>Wango</rdfs:label>
    </owl:NamedIndividual>
    


    <!-- http://purl.obolibrary.org/obo/GAZ_00255773 -->

    <owl:NamedIndividual rdf:about="http://purl.obolibrary.org/obo/GAZ_00255773">
        <obo:RO_0001025 rdf:resource="http://purl.obolibrary.org/obo/GAZ_00009134"/>
        <obo:IAO_0000115>A populated place.</obo:IAO_0000115>
        <oboInOwl:hasOBONamespace>GAZ</oboInOwl:hasOBONamespace>
        <oboInOwl:id>GAZ:00255773</oboInOwl:id>
        <rdfs:label>Apaora</rdfs:label>
    </owl:NamedIndividual>
    


    <!-- http://purl.obolibrary.org/obo/GAZ_00255774 -->

    <owl:NamedIndividual rdf:about="http://purl.obolibrary.org/obo/GAZ_00255774">
        <obo:RO_0001025 rdf:resource="http://purl.obolibrary.org/obo/GAZ_00009134"/>
        <obo:IAO_0000115>The provincial capital of the Makira-Ulawa Province in the Solomon Islands.</obo:IAO_0000115>
        <oboInOwl:hasOBONamespace>GAZ</oboInOwl:hasOBONamespace>
        <oboInOwl:id>GAZ:00255774</oboInOwl:id>
        <rdfs:label>Kirakira</rdfs:label>
    </owl:NamedIndividual>
    


    <!-- http://purl.obolibrary.org/obo/GAZ_00255775 -->

    <owl:NamedIndividual rdf:about="http://purl.obolibrary.org/obo/GAZ_00255775">
        <obo:RO_0001025 rdf:resource="http://purl.obolibrary.org/obo/GAZ_00009134"/>
        <obo:IAO_0000115>A populated place.</obo:IAO_0000115>
        <oboInOwl:hasOBONamespace>GAZ</oboInOwl:hasOBONamespace>
        <oboInOwl:id>GAZ:00255775</oboInOwl:id>
        <rdfs:label>Naparenawa</rdfs:label>
    </owl:NamedIndividual>
    


    <!-- http://purl.obolibrary.org/obo/GAZ_00255776 -->

    <owl:NamedIndividual rdf:about="http://purl.obolibrary.org/obo/GAZ_00255776">
        <obo:RO_0001025 rdf:resource="http://purl.obolibrary.org/obo/GAZ_00009134"/>
        <obo:IAO_0000115>A populated place.</obo:IAO_0000115>
        <oboInOwl:hasOBONamespace>GAZ</oboInOwl:hasOBONamespace>
        <oboInOwl:id>GAZ:00255776</oboInOwl:id>
        <rdfs:label>Naana</rdfs:label>
    </owl:NamedIndividual>
    


    <!-- http://purl.obolibrary.org/obo/GAZ_00255777 -->

    <owl:NamedIndividual rdf:about="http://purl.obolibrary.org/obo/GAZ_00255777">
        <obo:RO_0001025 rdf:resource="http://purl.obolibrary.org/obo/GAZ_00009134"/>
        <obo:IAO_0000115>A populated place.</obo:IAO_0000115>
        <oboInOwl:hasOBONamespace>GAZ</oboInOwl:hasOBONamespace>
        <oboInOwl:id>GAZ:00255777</oboInOwl:id>
        <rdfs:label>Iaru</rdfs:label>
    </owl:NamedIndividual>
    


    <!-- http://purl.obolibrary.org/obo/GAZ_00255778 -->

    <owl:NamedIndividual rdf:about="http://purl.obolibrary.org/obo/GAZ_00255778">
        <obo:RO_0001025 rdf:resource="http://purl.obolibrary.org/obo/GAZ_00009134"/>
        <obo:IAO_0000115>A populated place.</obo:IAO_0000115>
        <oboInOwl:hasOBONamespace>GAZ</oboInOwl:hasOBONamespace>
        <oboInOwl:id>GAZ:00255778</oboInOwl:id>
        <rdfs:label>Manighai</rdfs:label>
    </owl:NamedIndividual>
    


    <!-- http://purl.obolibrary.org/obo/GAZ_00255779 -->

    <owl:NamedIndividual rdf:about="http://purl.obolibrary.org/obo/GAZ_00255779">
        <obo:RO_0001025 rdf:resource="http://purl.obolibrary.org/obo/GAZ_00009139"/>
        <obo:IAO_0000115>A populated place.</obo:IAO_0000115>
        <oboInOwl:hasOBONamespace>GAZ</oboInOwl:hasOBONamespace>
        <oboInOwl:id>GAZ:00255779</oboInOwl:id>
        <rdfs:label>Su&apos;ena</rdfs:label>
    </owl:NamedIndividual>
    


    <!-- http://purl.obolibrary.org/obo/GAZ_00255780 -->

    <owl:NamedIndividual rdf:about="http://purl.obolibrary.org/obo/GAZ_00255780">
        <obo:RO_0001025 rdf:resource="http://purl.obolibrary.org/obo/GAZ_00012779"/>
        <obo:IAO_0000115>Three island NE of Makira Island.</obo:IAO_0000115>
        <oboInOwl:hasOBONamespace>GAZ</oboInOwl:hasOBONamespace>
        <oboInOwl:id>GAZ:00255780</oboInOwl:id>
        <rdfs:label>Three Sisters Islands</rdfs:label>
    </owl:NamedIndividual>
    


    <!-- http://purl.obolibrary.org/obo/GAZ_00255781 -->

    <owl:NamedIndividual rdf:about="http://purl.obolibrary.org/obo/GAZ_00255781">
        <obo:RO_0001025 rdf:resource="http://purl.obolibrary.org/obo/GAZ_00012779"/>
        <obo:IAO_0000115>An island in the Solomon Islands; it is located in Makira-Ulawa Province.</obo:IAO_0000115>
        <oboInOwl:hasOBONamespace>GAZ</oboInOwl:hasOBONamespace>
        <oboInOwl:id>GAZ:00255781</oboInOwl:id>
        <rdfs:label>Ali&apos;ite Island</rdfs:label>
    </owl:NamedIndividual>
    


    <!-- http://purl.obolibrary.org/obo/GAZ_00255782 -->

    <owl:NamedIndividual rdf:about="http://purl.obolibrary.org/obo/GAZ_00255782">
        <obo:RO_0001025 rdf:resource="http://purl.obolibrary.org/obo/GAZ_00009137"/>
        <obo:IAO_0000115>A populated place. The provincial capital of Malaita Province, Solomon Islands. It is situated on the northern end of Langalanga Lagoon on the north-west coast of Malaita Island.</obo:IAO_0000115>
        <oboInOwl:hasOBONamespace>GAZ</oboInOwl:hasOBONamespace>
        <oboInOwl:id>GAZ:00255782</oboInOwl:id>
        <rdfs:label>Auki</rdfs:label>
    </owl:NamedIndividual>
    


    <!-- http://purl.obolibrary.org/obo/GAZ_00255783 -->

    <owl:NamedIndividual rdf:about="http://purl.obolibrary.org/obo/GAZ_00255783">
        <obo:RO_0001025 rdf:resource="http://purl.obolibrary.org/obo/GAZ_00255745"/>
        <obo:IAO_0000115>A coral reef.</obo:IAO_0000115>
        <oboInOwl:hasOBONamespace>GAZ</oboInOwl:hasOBONamespace>
        <oboInOwl:id>GAZ:00255783</oboInOwl:id>
        <rdfs:label>Indispensable Reef Middle</rdfs:label>
    </owl:NamedIndividual>
    


    <!-- http://purl.obolibrary.org/obo/GAZ_00255784 -->

    <owl:NamedIndividual rdf:about="http://purl.obolibrary.org/obo/GAZ_00255784">
        <obo:RO_0001025 rdf:resource="http://purl.obolibrary.org/obo/GAZ_00049018"/>
        <obo:IAO_0000115>A populated place.</obo:IAO_0000115>
        <oboInOwl:hasOBONamespace>GAZ</oboInOwl:hasOBONamespace>
        <oboInOwl:id>GAZ:00255784</oboInOwl:id>
        <rdfs:label>Mahuto</rdfs:label>
    </owl:NamedIndividual>
    


    <!-- http://purl.obolibrary.org/obo/GAZ_00255785 -->

    <owl:NamedIndividual rdf:about="http://purl.obolibrary.org/obo/GAZ_00255785">
        <obo:RO_0001025 rdf:resource="http://purl.obolibrary.org/obo/GAZ_00049018"/>
        <obo:IAO_0000115>A populated place.</obo:IAO_0000115>
        <oboInOwl:hasOBONamespace>GAZ</oboInOwl:hasOBONamespace>
        <oboInOwl:id>GAZ:00255785</oboInOwl:id>
        <rdfs:label>Heraniesi</rdfs:label>
    </owl:NamedIndividual>
    


    <!-- http://purl.obolibrary.org/obo/GAZ_00255786 -->

    <owl:NamedIndividual rdf:about="http://purl.obolibrary.org/obo/GAZ_00255786">
        <obo:RO_0001025 rdf:resource="http://purl.obolibrary.org/obo/GAZ_00049018"/>
        <obo:IAO_0000115>A populated place.</obo:IAO_0000115>
        <oboInOwl:hasOBONamespace>GAZ</oboInOwl:hasOBONamespace>
        <oboInOwl:id>GAZ:00255786</oboInOwl:id>
        <rdfs:label>Sarawasi</rdfs:label>
    </owl:NamedIndividual>
    


    <!-- http://purl.obolibrary.org/obo/GAZ_00255787 -->

    <owl:NamedIndividual rdf:about="http://purl.obolibrary.org/obo/GAZ_00255787">
        <obo:RO_0001025 rdf:resource="http://purl.obolibrary.org/obo/GAZ_00049018"/>
        <obo:IAO_0000115>A populated place.</obo:IAO_0000115>
        <oboInOwl:hasOBONamespace>GAZ</oboInOwl:hasOBONamespace>
        <oboInOwl:id>GAZ:00255787</oboInOwl:id>
        <rdfs:label>Wailulu</rdfs:label>
    </owl:NamedIndividual>
    


    <!-- http://purl.obolibrary.org/obo/GAZ_00255788 -->

    <owl:NamedIndividual rdf:about="http://purl.obolibrary.org/obo/GAZ_00255788">
        <obo:RO_0001025 rdf:resource="http://purl.obolibrary.org/obo/GAZ_00049018"/>
        <obo:IAO_0000115>A populated place.</obo:IAO_0000115>
        <oboInOwl:hasOBONamespace>GAZ</oboInOwl:hasOBONamespace>
        <oboInOwl:id>GAZ:00255788</oboInOwl:id>
        <rdfs:label>Heupeine</rdfs:label>
    </owl:NamedIndividual>
    


    <!-- http://purl.obolibrary.org/obo/GAZ_00255789 -->

    <owl:NamedIndividual rdf:about="http://purl.obolibrary.org/obo/GAZ_00255789">
        <obo:RO_0001025 rdf:resource="http://purl.obolibrary.org/obo/GAZ_00049018"/>
        <obo:IAO_0000115>A populated place.</obo:IAO_0000115>
        <oboInOwl:hasOBONamespace>GAZ</oboInOwl:hasOBONamespace>
        <oboInOwl:id>GAZ:00255789</oboInOwl:id>
        <rdfs:label>Sa&apos;a</rdfs:label>
    </owl:NamedIndividual>
    


    <!-- http://purl.obolibrary.org/obo/GAZ_00255790 -->

    <owl:NamedIndividual rdf:about="http://purl.obolibrary.org/obo/GAZ_00255790">
        <obo:RO_0001025 rdf:resource="http://purl.obolibrary.org/obo/GAZ_00049018"/>
        <obo:IAO_0000115>A populated place.</obo:IAO_0000115>
        <oboInOwl:hasOBONamespace>GAZ</oboInOwl:hasOBONamespace>
        <oboInOwl:id>GAZ:00255790</oboInOwl:id>
        <rdfs:label>Palasu&apos;u</rdfs:label>
    </owl:NamedIndividual>
    


    <!-- http://purl.obolibrary.org/obo/GAZ_00255791 -->

    <owl:NamedIndividual rdf:about="http://purl.obolibrary.org/obo/GAZ_00255791">
        <obo:RO_0001025 rdf:resource="http://purl.obolibrary.org/obo/GAZ_00007203"/>
        <obo:IAO_0000115>An island on Ontong Java Atoll.</obo:IAO_0000115>
        <oboInOwl:hasOBONamespace>GAZ</oboInOwl:hasOBONamespace>
        <oboInOwl:id>GAZ:00255791</oboInOwl:id>
        <rdfs:label>Okarore</rdfs:label>
    </owl:NamedIndividual>
    


    <!-- http://purl.obolibrary.org/obo/GAZ_00255792 -->

    <owl:NamedIndividual rdf:about="http://purl.obolibrary.org/obo/GAZ_00255792">
        <obo:RO_0001025 rdf:resource="http://purl.obolibrary.org/obo/GAZ_00007203"/>
        <obo:IAO_0000115>An island on Ontong Java Atoll.</obo:IAO_0000115>
        <oboInOwl:hasOBONamespace>GAZ</oboInOwl:hasOBONamespace>
        <oboInOwl:id>GAZ:00255792</oboInOwl:id>
        <rdfs:label>Kapei</rdfs:label>
    </owl:NamedIndividual>
    


    <!-- http://purl.obolibrary.org/obo/GAZ_00255793 -->

    <owl:NamedIndividual rdf:about="http://purl.obolibrary.org/obo/GAZ_00255793">
        <obo:RO_0001025 rdf:resource="http://purl.obolibrary.org/obo/GAZ_00007203"/>
        <obo:IAO_0000115>An island on Ontong Java Atoll.</obo:IAO_0000115>
        <oboInOwl:hasOBONamespace>GAZ</oboInOwl:hasOBONamespace>
        <oboInOwl:id>GAZ:00255793</oboInOwl:id>
        <rdfs:label>Nguhakai</rdfs:label>
    </owl:NamedIndividual>
    


    <!-- http://purl.obolibrary.org/obo/GAZ_00255794 -->

    <owl:NamedIndividual rdf:about="http://purl.obolibrary.org/obo/GAZ_00255794">
        <obo:RO_0001025 rdf:resource="http://purl.obolibrary.org/obo/GAZ_00007203"/>
        <obo:IAO_0000115>An island on Ontong Java Atoll.</obo:IAO_0000115>
        <oboInOwl:hasOBONamespace>GAZ</oboInOwl:hasOBONamespace>
        <oboInOwl:id>GAZ:00255794</oboInOwl:id>
        <rdfs:label>Kengou</rdfs:label>
    </owl:NamedIndividual>
    


    <!-- http://purl.obolibrary.org/obo/GAZ_00255795 -->

    <owl:NamedIndividual rdf:about="http://purl.obolibrary.org/obo/GAZ_00255795">
        <obo:RO_0001025 rdf:resource="http://purl.obolibrary.org/obo/GAZ_00007203"/>
        <obo:IAO_0000115>An island on Ontong Java Atoll.</obo:IAO_0000115>
        <oboInOwl:hasOBONamespace>GAZ</oboInOwl:hasOBONamespace>
        <oboInOwl:id>GAZ:00255795</oboInOwl:id>
        <rdfs:label>Kekumounga</rdfs:label>
    </owl:NamedIndividual>
    


    <!-- http://purl.obolibrary.org/obo/GAZ_00255796 -->

    <owl:NamedIndividual rdf:about="http://purl.obolibrary.org/obo/GAZ_00255796">
        <obo:RO_0001025 rdf:resource="http://purl.obolibrary.org/obo/GAZ_00007203"/>
        <obo:IAO_0000115>An island on Ontong Java Atoll.</obo:IAO_0000115>
        <oboInOwl:hasOBONamespace>GAZ</oboInOwl:hasOBONamespace>
        <oboInOwl:id>GAZ:00255796</oboInOwl:id>
        <rdfs:label>Opaha</rdfs:label>
    </owl:NamedIndividual>
    


    <!-- http://purl.obolibrary.org/obo/GAZ_00255797 -->

    <owl:NamedIndividual rdf:about="http://purl.obolibrary.org/obo/GAZ_00255797">
        <obo:RO_0001025 rdf:resource="http://purl.obolibrary.org/obo/GAZ_00007203"/>
        <obo:IAO_0000115>An island on Ontong Java Atoll.</obo:IAO_0000115>
        <oboInOwl:hasOBONamespace>GAZ</oboInOwl:hasOBONamespace>
        <oboInOwl:id>GAZ:00255797</oboInOwl:id>
        <rdfs:label>Keila</rdfs:label>
    </owl:NamedIndividual>
    


    <!-- http://purl.obolibrary.org/obo/GAZ_00255798 -->

    <owl:NamedIndividual rdf:about="http://purl.obolibrary.org/obo/GAZ_00255798">
        <obo:RO_0001025 rdf:resource="http://purl.obolibrary.org/obo/GAZ_00016915"/>
        <obo:IAO_0000115>An island on Ontong Java Atoll.</obo:IAO_0000115>
        <oboInOwl:hasOBONamespace>GAZ</oboInOwl:hasOBONamespace>
        <oboInOwl:id>GAZ:00255798</oboInOwl:id>
        <rdfs:label>Tehaolei Island</rdfs:label>
    </owl:NamedIndividual>
    


    <!-- http://purl.obolibrary.org/obo/GAZ_00255799 -->

    <owl:NamedIndividual rdf:about="http://purl.obolibrary.org/obo/GAZ_00255799">
        <obo:RO_0001025 rdf:resource="http://purl.obolibrary.org/obo/GAZ_00007203"/>
        <obo:IAO_0000115>An island on Ontong Java Atoll.</obo:IAO_0000115>
        <oboInOwl:hasOBONamespace>GAZ</oboInOwl:hasOBONamespace>
        <oboInOwl:id>GAZ:00255799</oboInOwl:id>
        <rdfs:label>Keuolei</rdfs:label>
    </owl:NamedIndividual>
    


    <!-- http://purl.obolibrary.org/obo/GAZ_00255800 -->

    <owl:NamedIndividual rdf:about="http://purl.obolibrary.org/obo/GAZ_00255800">
        <obo:RO_0001025 rdf:resource="http://purl.obolibrary.org/obo/GAZ_00007203"/>
        <obo:IAO_0000115>An island on Ontong Java Atoll.</obo:IAO_0000115>
        <oboInOwl:hasOBONamespace>GAZ</oboInOwl:hasOBONamespace>
        <oboInOwl:id>GAZ:00255800</oboInOwl:id>
        <rdfs:label>Kehango</rdfs:label>
    </owl:NamedIndividual>
    


    <!-- http://purl.obolibrary.org/obo/GAZ_00255801 -->

    <owl:NamedIndividual rdf:about="http://purl.obolibrary.org/obo/GAZ_00255801">
        <obo:RO_0001025 rdf:resource="http://purl.obolibrary.org/obo/GAZ_00007203"/>
        <obo:IAO_0000115>An island on Ontong Java Atoll.</obo:IAO_0000115>
        <oboInOwl:hasOBONamespace>GAZ</oboInOwl:hasOBONamespace>
        <oboInOwl:id>GAZ:00255801</oboInOwl:id>
        <rdfs:label>Oko</rdfs:label>
    </owl:NamedIndividual>
    


    <!-- http://purl.obolibrary.org/obo/GAZ_00255802 -->

    <owl:NamedIndividual rdf:about="http://purl.obolibrary.org/obo/GAZ_00255802">
        <obo:RO_0001025 rdf:resource="http://purl.obolibrary.org/obo/GAZ_00007203"/>
        <obo:IAO_0000115>An island on Ontong Java Atoll.</obo:IAO_0000115>
        <oboInOwl:hasOBONamespace>GAZ</oboInOwl:hasOBONamespace>
        <oboInOwl:id>GAZ:00255802</oboInOwl:id>
        <rdfs:label>Ouku</rdfs:label>
    </owl:NamedIndividual>
    


    <!-- http://purl.obolibrary.org/obo/GAZ_00255803 -->

    <owl:NamedIndividual rdf:about="http://purl.obolibrary.org/obo/GAZ_00255803">
        <obo:RO_0001025 rdf:resource="http://purl.obolibrary.org/obo/GAZ_00007203"/>
        <obo:IAO_0000115>An island on Ontong Java Atoll.</obo:IAO_0000115>
        <oboInOwl:hasOBONamespace>GAZ</oboInOwl:hasOBONamespace>
        <oboInOwl:id>GAZ:00255803</oboInOwl:id>
        <rdfs:label>Hengualoko</rdfs:label>
    </owl:NamedIndividual>
    


    <!-- http://purl.obolibrary.org/obo/GAZ_00255804 -->

    <owl:NamedIndividual rdf:about="http://purl.obolibrary.org/obo/GAZ_00255804">
        <obo:RO_0001025 rdf:resource="http://purl.obolibrary.org/obo/GAZ_00007203"/>
        <obo:IAO_0000115>An island on Ontong Java Atoll.</obo:IAO_0000115>
        <oboInOwl:hasOBONamespace>GAZ</oboInOwl:hasOBONamespace>
        <oboInOwl:id>GAZ:00255804</oboInOwl:id>
        <rdfs:label>Henguakaha</rdfs:label>
    </owl:NamedIndividual>
    


    <!-- http://purl.obolibrary.org/obo/GAZ_00255805 -->

    <owl:NamedIndividual rdf:about="http://purl.obolibrary.org/obo/GAZ_00255805">
        <obo:RO_0001025 rdf:resource="http://purl.obolibrary.org/obo/GAZ_00007203"/>
        <obo:IAO_0000115>An island on Ontong Java Atoll.</obo:IAO_0000115>
        <oboInOwl:hasOBONamespace>GAZ</oboInOwl:hasOBONamespace>
        <oboInOwl:id>GAZ:00255805</oboInOwl:id>
        <rdfs:label>Pei</rdfs:label>
    </owl:NamedIndividual>
    


    <!-- http://purl.obolibrary.org/obo/GAZ_00255806 -->

    <owl:NamedIndividual rdf:about="http://purl.obolibrary.org/obo/GAZ_00255806">
        <obo:RO_0001025 rdf:resource="http://purl.obolibrary.org/obo/GAZ_00007203"/>
        <obo:IAO_0000115>An island on Ontong Java Atoll.</obo:IAO_0000115>
        <oboInOwl:hasOBONamespace>GAZ</oboInOwl:hasOBONamespace>
        <oboInOwl:id>GAZ:00255806</oboInOwl:id>
        <rdfs:label>Kukolu</rdfs:label>
    </owl:NamedIndividual>
    


    <!-- http://purl.obolibrary.org/obo/GAZ_00255807 -->

    <owl:NamedIndividual rdf:about="http://purl.obolibrary.org/obo/GAZ_00255807">
        <obo:RO_0001025 rdf:resource="http://purl.obolibrary.org/obo/GAZ_00016915"/>
        <obo:IAO_0000115>An island.</obo:IAO_0000115>
        <oboInOwl:hasOBONamespace>GAZ</oboInOwl:hasOBONamespace>
        <oboInOwl:id>GAZ:00255807</oboInOwl:id>
        <rdfs:label>Matuiloto Island</rdfs:label>
    </owl:NamedIndividual>
    


    <!-- http://purl.obolibrary.org/obo/GAZ_00255808 -->

    <owl:NamedIndividual rdf:about="http://purl.obolibrary.org/obo/GAZ_00255808">
        <obo:RO_0001025 rdf:resource="http://purl.obolibrary.org/obo/GAZ_00016915"/>
        <obo:IAO_0000115>The lagoon of Sikaiana Atoll.</obo:IAO_0000115>
        <oboInOwl:hasOBONamespace>GAZ</oboInOwl:hasOBONamespace>
        <oboInOwl:id>GAZ:00255808</oboInOwl:id>
        <rdfs:label>Te Moana</rdfs:label>
    </owl:NamedIndividual>
    


    <!-- http://purl.obolibrary.org/obo/GAZ_00255809 -->

    <owl:NamedIndividual rdf:about="http://purl.obolibrary.org/obo/GAZ_00255809">
        <obo:RO_0001025 rdf:resource="http://purl.obolibrary.org/obo/GAZ_00016915"/>
        <obo:IAO_0000115>An artificial island.</obo:IAO_0000115>
        <oboInOwl:hasOBONamespace>GAZ</oboInOwl:hasOBONamespace>
        <oboInOwl:id>GAZ:00255809</oboInOwl:id>
        <rdfs:label>Te Palena</rdfs:label>
    </owl:NamedIndividual>
    


    <!-- http://purl.obolibrary.org/obo/GAZ_00255810 -->

    <owl:NamedIndividual rdf:about="http://purl.obolibrary.org/obo/GAZ_00255810">
        <obo:RO_0001025 rdf:resource="http://purl.obolibrary.org/obo/GAZ_00016915"/>
        <obo:IAO_0000115>An artificial island.</obo:IAO_0000115>
        <oboInOwl:hasOBONamespace>GAZ</oboInOwl:hasOBONamespace>
        <oboInOwl:id>GAZ:00255810</oboInOwl:id>
        <rdfs:label>Hakatai&apos;atata</rdfs:label>
    </owl:NamedIndividual>
    


    <!-- http://purl.obolibrary.org/obo/GAZ_00255811 -->

    <owl:NamedIndividual rdf:about="http://purl.obolibrary.org/obo/GAZ_00255811">
        <obo:RO_0001025 rdf:resource="http://purl.obolibrary.org/obo/GAZ_00009558"/>
        <obo:IAO_0000115>An island in the Solomon Islands; it is located in Malaita Province.</obo:IAO_0000115>
        <oboInOwl:hasOBONamespace>GAZ</oboInOwl:hasOBONamespace>
        <oboInOwl:id>GAZ:00255811</oboInOwl:id>
        <rdfs:label>Sulufou Island</rdfs:label>
    </owl:NamedIndividual>
    


    <!-- http://purl.obolibrary.org/obo/GAZ_00255812 -->

    <owl:NamedIndividual rdf:about="http://purl.obolibrary.org/obo/GAZ_00255812">
        <obo:RO_0001025 rdf:resource="http://purl.obolibrary.org/obo/GAZ_00009558"/>
        <obo:IAO_0000115>An island in the Solomon Islands; it is located in Malaita Province.</obo:IAO_0000115>
        <oboInOwl:hasOBONamespace>GAZ</oboInOwl:hasOBONamespace>
        <oboInOwl:id>GAZ:00255812</oboInOwl:id>
        <rdfs:label>Mbasakana ·Island</rdfs:label>
    </owl:NamedIndividual>
    


    <!-- http://purl.obolibrary.org/obo/GAZ_00255813 -->

    <owl:NamedIndividual rdf:about="http://purl.obolibrary.org/obo/GAZ_00255813">
        <obo:RO_0001025 rdf:resource="http://purl.obolibrary.org/obo/GAZ_00009558"/>
        <obo:IAO_0000115>An island in the Solomon Islands; it is located in Malaita Province.</obo:IAO_0000115>
        <oboInOwl:hasOBONamespace>GAZ</oboInOwl:hasOBONamespace>
        <oboInOwl:id>GAZ:00255813</oboInOwl:id>
        <rdfs:label>Ndai Island</rdfs:label>
    </owl:NamedIndividual>
    


    <!-- http://purl.obolibrary.org/obo/GAZ_00255814 -->

    <owl:NamedIndividual rdf:about="http://purl.obolibrary.org/obo/GAZ_00255814">
        <obo:RO_0001025 rdf:resource="http://purl.obolibrary.org/obo/GAZ_00009558"/>
        <obo:IAO_0000115>An island in the Solomon Islands; it is located in Malaita Province.</obo:IAO_0000115>
        <oboInOwl:hasOBONamespace>GAZ</oboInOwl:hasOBONamespace>
        <oboInOwl:id>GAZ:00255814</oboInOwl:id>
        <rdfs:label>Maana&apos;omba Island</rdfs:label>
    </owl:NamedIndividual>
    


    <!-- http://purl.obolibrary.org/obo/GAZ_00255815 -->

    <owl:NamedIndividual rdf:about="http://purl.obolibrary.org/obo/GAZ_00255815">
        <obo:RO_0001025 rdf:resource="http://purl.obolibrary.org/obo/GAZ_00255821"/>
        <obo:IAO_0000115>An artificial island in the Langa Langa Lagoon, South of Auki on the island of Malaita in the Solomon Islands.</obo:IAO_0000115>
        <oboInOwl:hasOBONamespace>GAZ</oboInOwl:hasOBONamespace>
        <oboInOwl:id>GAZ:00255815</oboInOwl:id>
        <rdfs:label>Laulasi Island</rdfs:label>
    </owl:NamedIndividual>
    


    <!-- http://purl.obolibrary.org/obo/GAZ_00255816 -->

    <owl:NamedIndividual rdf:about="http://purl.obolibrary.org/obo/GAZ_00255816">
        <obo:RO_0001025 rdf:resource="http://purl.obolibrary.org/obo/GAZ_00009558"/>
        <oboInOwl:hasOBONamespace>GAZ</oboInOwl:hasOBONamespace>
        <oboInOwl:id>GAZ:00255816</oboInOwl:id>
        <rdfs:label>Adagege Island</rdfs:label>
    </owl:NamedIndividual>
    


    <!-- http://purl.obolibrary.org/obo/GAZ_00255817 -->

    <owl:NamedIndividual rdf:about="http://purl.obolibrary.org/obo/GAZ_00255817">
        <obo:RO_0001025 rdf:resource="http://purl.obolibrary.org/obo/GAZ_00009558"/>
        <obo:IAO_0000115>An island in the Solomon Islands; it is located in Malaita Province.</obo:IAO_0000115>
        <oboInOwl:hasOBONamespace>GAZ</oboInOwl:hasOBONamespace>
        <oboInOwl:id>GAZ:00255817</oboInOwl:id>
        <rdfs:label>Alite Island</rdfs:label>
    </owl:NamedIndividual>
    


    <!-- http://purl.obolibrary.org/obo/GAZ_00255818 -->

    <owl:NamedIndividual rdf:about="http://purl.obolibrary.org/obo/GAZ_00255818">
        <obo:RO_0001025 rdf:resource="http://purl.obolibrary.org/obo/GAZ_00009558"/>
        <obo:IAO_0000115>An island in the Solomon Islands; it is located in Malaita Province.</obo:IAO_0000115>
        <oboInOwl:hasOBONamespace>GAZ</oboInOwl:hasOBONamespace>
        <oboInOwl:id>GAZ:00255818</oboInOwl:id>
        <rdfs:label>Anuta Paina Island</rdfs:label>
    </owl:NamedIndividual>
    


    <!-- http://purl.obolibrary.org/obo/GAZ_00255819 -->

    <owl:NamedIndividual rdf:about="http://purl.obolibrary.org/obo/GAZ_00255819">
        <obo:RO_0001025 rdf:resource="http://purl.obolibrary.org/obo/GAZ_00255820"/>
        <obo:IAO_0000115>An island in the Lau Lagoon off the northeast coast of Malaita Island.</obo:IAO_0000115>
        <oboInOwl:hasOBONamespace>GAZ</oboInOwl:hasOBONamespace>
        <oboInOwl:id>GAZ:00255819</oboInOwl:id>
        <rdfs:label>Funaafou Island</rdfs:label>
    </owl:NamedIndividual>
    


    <!-- http://purl.obolibrary.org/obo/GAZ_00255820 -->

    <owl:NamedIndividual rdf:about="http://purl.obolibrary.org/obo/GAZ_00255820">
        <obo:RO_0001025 rdf:resource="http://purl.obolibrary.org/obo/GAZ_00009137"/>
        <obo:IAO_0000115>A lagoon located on the north east coast of Malaita Island.</obo:IAO_0000115>
        <oboInOwl:hasOBONamespace>GAZ</oboInOwl:hasOBONamespace>
        <oboInOwl:id>GAZ:00255820</oboInOwl:id>
        <rdfs:label>Lau Lagoon</rdfs:label>
    </owl:NamedIndividual>
    


    <!-- http://purl.obolibrary.org/obo/GAZ_00255821 -->

    <owl:NamedIndividual rdf:about="http://purl.obolibrary.org/obo/GAZ_00255821">
        <obo:RO_0001025 rdf:resource="http://purl.obolibrary.org/obo/GAZ_00009137"/>
        <obo:IAO_0000115>A natural lagoon on the West coast of Malaita near the provincial capital Auki within the Solomon Islands.</obo:IAO_0000115>
        <oboInOwl:hasOBONamespace>GAZ</oboInOwl:hasOBONamespace>
        <oboInOwl:id>GAZ:00255821</oboInOwl:id>
        <rdfs:label>Langa Langa Lagoon</rdfs:label>
    </owl:NamedIndividual>
    


    <!-- http://purl.obolibrary.org/obo/GAZ_00255822 -->

    <owl:NamedIndividual rdf:about="http://purl.obolibrary.org/obo/GAZ_00255822">
        <obo:RO_0001025 rdf:resource="http://purl.obolibrary.org/obo/GAZ_00007206"/>
        <obo:IAO_0000115>A populated place.</obo:IAO_0000115>
        <oboInOwl:hasOBONamespace>GAZ</oboInOwl:hasOBONamespace>
        <oboInOwl:id>GAZ:00255822</oboInOwl:id>
        <rdfs:label>Manggautu</rdfs:label>
    </owl:NamedIndividual>
    


    <!-- http://purl.obolibrary.org/obo/GAZ_00255823 -->

    <owl:NamedIndividual rdf:about="http://purl.obolibrary.org/obo/GAZ_00255823">
        <rdf:type rdf:resource="http://purl.obolibrary.org/obo/ENVO_00000856"/>
        <obo:RO_0001025 rdf:resource="http://purl.obolibrary.org/obo/GAZ_00007206"/>
        <obo:IAO_0000115>A populated place. A village.</obo:IAO_0000115>
        <oboInOwl:hasOBONamespace>GAZ</oboInOwl:hasOBONamespace>
        <oboInOwl:id>GAZ:00255823</oboInOwl:id>
        <rdfs:label>Kangua</rdfs:label>
    </owl:NamedIndividual>
    


    <!-- http://purl.obolibrary.org/obo/GAZ_00255824 -->

    <owl:NamedIndividual rdf:about="http://purl.obolibrary.org/obo/GAZ_00255824">
        <rdf:type rdf:resource="http://purl.obolibrary.org/obo/ENVO_00000856"/>
        <obo:RO_0001025 rdf:resource="http://purl.obolibrary.org/obo/GAZ_00007206"/>
        <obo:IAO_0000115>A populated place. A village in the Solomon Islands, on Rennell Island. It is the capital of Rennell and Bellona province.</obo:IAO_0000115>
        <oboInOwl:hasOBONamespace>GAZ</oboInOwl:hasOBONamespace>
        <oboInOwl:id>GAZ:00255824</oboInOwl:id>
        <rdfs:label>Tingoa</rdfs:label>
    </owl:NamedIndividual>
    


    <!-- http://purl.obolibrary.org/obo/GAZ_00255825 -->

    <owl:NamedIndividual rdf:about="http://purl.obolibrary.org/obo/GAZ_00255825">
        <rdf:type rdf:resource="http://purl.obolibrary.org/obo/ENVO_00000856"/>
        <obo:RO_0001025 rdf:resource="http://purl.obolibrary.org/obo/GAZ_00007206"/>
        <obo:IAO_0000115>A populated place. A village in the Solomon Islands, on Rennell Island in the Rennell and Bellona province.</obo:IAO_0000115>
        <oboInOwl:hasOBONamespace>GAZ</oboInOwl:hasOBONamespace>
        <oboInOwl:id>GAZ:00255825</oboInOwl:id>
        <rdfs:label>Tahanuku</rdfs:label>
    </owl:NamedIndividual>
    


    <!-- http://purl.obolibrary.org/obo/GAZ_00255826 -->

    <owl:NamedIndividual rdf:about="http://purl.obolibrary.org/obo/GAZ_00255826">
        <rdf:type rdf:resource="http://purl.obolibrary.org/obo/ENVO_00000856"/>
        <obo:RO_0001025 rdf:resource="http://purl.obolibrary.org/obo/GAZ_00007206"/>
        <obo:IAO_0000115>A populated place. A village.</obo:IAO_0000115>
        <oboInOwl:hasOBONamespace>GAZ</oboInOwl:hasOBONamespace>
        <oboInOwl:id>GAZ:00255826</oboInOwl:id>
        <rdfs:label>Lughughi</rdfs:label>
    </owl:NamedIndividual>
    


    <!-- http://purl.obolibrary.org/obo/GAZ_00255827 -->

    <owl:NamedIndividual rdf:about="http://purl.obolibrary.org/obo/GAZ_00255827">
        <rdf:type rdf:resource="http://purl.obolibrary.org/obo/ENVO_00000856"/>
        <obo:RO_0001025 rdf:resource="http://purl.obolibrary.org/obo/GAZ_00007206"/>
        <obo:IAO_0000115>A populated place. A village.</obo:IAO_0000115>
        <oboInOwl:hasOBONamespace>GAZ</oboInOwl:hasOBONamespace>
        <oboInOwl:id>GAZ:00255827</oboInOwl:id>
        <rdfs:label>Matangi</rdfs:label>
    </owl:NamedIndividual>
    


    <!-- http://purl.obolibrary.org/obo/GAZ_00255828 -->

    <owl:NamedIndividual rdf:about="http://purl.obolibrary.org/obo/GAZ_00255828">
        <rdf:type rdf:resource="http://purl.obolibrary.org/obo/ENVO_00000856"/>
        <obo:RO_0001025 rdf:resource="http://purl.obolibrary.org/obo/GAZ_00007206"/>
        <obo:IAO_0000115>A populated place. A village.</obo:IAO_0000115>
        <oboInOwl:hasOBONamespace>GAZ</oboInOwl:hasOBONamespace>
        <oboInOwl:id>GAZ:00255828</oboInOwl:id>
        <rdfs:label>Kanava</rdfs:label>
    </owl:NamedIndividual>
    


    <!-- http://purl.obolibrary.org/obo/GAZ_00255829 -->

    <owl:NamedIndividual rdf:about="http://purl.obolibrary.org/obo/GAZ_00255829">
        <rdf:type rdf:resource="http://purl.obolibrary.org/obo/ENVO_00000856"/>
        <obo:RO_0001025 rdf:resource="http://purl.obolibrary.org/obo/GAZ_00007206"/>
        <obo:IAO_0000115>A populated place. A village in the Solomon Islands, on Rennell Island in the Rennell and Bellona province.</obo:IAO_0000115>
        <oboInOwl:hasOBONamespace>GAZ</oboInOwl:hasOBONamespace>
        <oboInOwl:id>GAZ:00255829</oboInOwl:id>
        <rdfs:label>Lavangu</rdfs:label>
    </owl:NamedIndividual>
    


    <!-- http://purl.obolibrary.org/obo/GAZ_00255830 -->

    <owl:NamedIndividual rdf:about="http://purl.obolibrary.org/obo/GAZ_00255830">
        <rdf:type rdf:resource="http://purl.obolibrary.org/obo/ENVO_00000856"/>
        <obo:RO_0001025 rdf:resource="http://purl.obolibrary.org/obo/GAZ_00007206"/>
        <obo:IAO_0000115>A populated place. A village.</obo:IAO_0000115>
        <oboInOwl:hasOBONamespace>GAZ</oboInOwl:hasOBONamespace>
        <oboInOwl:id>GAZ:00255830</oboInOwl:id>
        <rdfs:label>Kiakoe</rdfs:label>
    </owl:NamedIndividual>
    


    <!-- http://purl.obolibrary.org/obo/GAZ_00255831 -->

    <owl:NamedIndividual rdf:about="http://purl.obolibrary.org/obo/GAZ_00255831">
        <rdf:type rdf:resource="http://purl.obolibrary.org/obo/ENVO_00000856"/>
        <obo:RO_0001025 rdf:resource="http://purl.obolibrary.org/obo/GAZ_00007206"/>
        <obo:IAO_0000115>A populated place. A village.</obo:IAO_0000115>
        <oboInOwl:hasOBONamespace>GAZ</oboInOwl:hasOBONamespace>
        <oboInOwl:id>GAZ:00255831</oboInOwl:id>
        <rdfs:label>Tenggano</rdfs:label>
    </owl:NamedIndividual>
    


    <!-- http://purl.obolibrary.org/obo/GAZ_00255832 -->

    <owl:NamedIndividual rdf:about="http://purl.obolibrary.org/obo/GAZ_00255832">
        <rdf:type rdf:resource="http://purl.obolibrary.org/obo/ENVO_00000856"/>
        <obo:RO_0001025 rdf:resource="http://purl.obolibrary.org/obo/GAZ_00007206"/>
        <obo:IAO_0000115>A populated place. A village in the Solomon Islands, on Rennell Island in the Rennell and Bellona province.</obo:IAO_0000115>
        <oboInOwl:hasOBONamespace>GAZ</oboInOwl:hasOBONamespace>
        <oboInOwl:id>GAZ:00255832</oboInOwl:id>
        <rdfs:label>Hutuna</rdfs:label>
    </owl:NamedIndividual>
    


    <!-- http://purl.obolibrary.org/obo/GAZ_00255833 -->

    <owl:NamedIndividual rdf:about="http://purl.obolibrary.org/obo/GAZ_00255833">
        <obo:RO_0001025 rdf:resource="http://purl.obolibrary.org/obo/GAZ_00007206"/>
        <obo:IAO_0000115>A bay on the SW coast of Rennell Island.</obo:IAO_0000115>
        <oboInOwl:hasOBONamespace>GAZ</oboInOwl:hasOBONamespace>
        <oboInOwl:id>GAZ:00255833</oboInOwl:id>
        <rdfs:label>Kangava Bay</rdfs:label>
    </owl:NamedIndividual>
    


    <!-- http://purl.obolibrary.org/obo/GAZ_00255834 -->

    <owl:NamedIndividual rdf:about="http://purl.obolibrary.org/obo/GAZ_00255834">
        <rdf:type rdf:resource="http://purl.obolibrary.org/obo/ENVO_00000856"/>
        <obo:RO_0001025 rdf:resource="http://purl.obolibrary.org/obo/GAZ_00016929"/>
        <obo:IAO_0000115>A populated place. A village.</obo:IAO_0000115>
        <oboInOwl:hasOBONamespace>GAZ</oboInOwl:hasOBONamespace>
        <oboInOwl:id>GAZ:00255834</oboInOwl:id>
        <rdfs:label>Matahenua/Matamoana</rdfs:label>
    </owl:NamedIndividual>
    


    <!-- http://purl.obolibrary.org/obo/GAZ_00255835 -->

    <owl:NamedIndividual rdf:about="http://purl.obolibrary.org/obo/GAZ_00255835">
        <rdf:type rdf:resource="http://purl.obolibrary.org/obo/ENVO_00000856"/>
        <obo:RO_0001025 rdf:resource="http://purl.obolibrary.org/obo/GAZ_00016929"/>
        <obo:IAO_0000115>A populated place. A village.</obo:IAO_0000115>
        <oboInOwl:hasOBONamespace>GAZ</oboInOwl:hasOBONamespace>
        <oboInOwl:id>GAZ:00255835</oboInOwl:id>
        <rdfs:label>Honga&apos;ubea</rdfs:label>
    </owl:NamedIndividual>
    


    <!-- http://purl.obolibrary.org/obo/GAZ_00255836 -->

    <owl:NamedIndividual rdf:about="http://purl.obolibrary.org/obo/GAZ_00255836">
        <obo:RO_0001025 rdf:resource="http://purl.obolibrary.org/obo/GAZ_00255745"/>
        <obo:IAO_0000115>A coral reef.</obo:IAO_0000115>
        <oboInOwl:hasOBONamespace>GAZ</oboInOwl:hasOBONamespace>
        <oboInOwl:id>GAZ:00255836</oboInOwl:id>
        <rdfs:label>Indispensable Reef South</rdfs:label>
    </owl:NamedIndividual>
    


    <!-- http://purl.obolibrary.org/obo/GAZ_00255837 -->

    <owl:NamedIndividual rdf:about="http://purl.obolibrary.org/obo/GAZ_00255837">
        <obo:RO_0001025 rdf:resource="http://purl.obolibrary.org/obo/GAZ_00255783"/>
        <obo:IAO_0000115>An island.</obo:IAO_0000115>
        <oboInOwl:hasOBONamespace>GAZ</oboInOwl:hasOBONamespace>
        <oboInOwl:id>GAZ:00255837</oboInOwl:id>
        <rdfs:label>Little Nottingham Islet</rdfs:label>
    </owl:NamedIndividual>
    


    <!-- http://purl.obolibrary.org/obo/GAZ_00255838 -->

    <owl:NamedIndividual rdf:about="http://purl.obolibrary.org/obo/GAZ_00255838">
        <rdf:type rdf:resource="http://purl.obolibrary.org/obo/ENVO_00000856"/>
        <obo:RO_0001025 rdf:resource="http://purl.obolibrary.org/obo/GAZ_00016929"/>
        <obo:IAO_0000115>A populated place. A village.</obo:IAO_0000115>
        <oboInOwl:hasOBONamespace>GAZ</oboInOwl:hasOBONamespace>
        <oboInOwl:id>GAZ:00255838</oboInOwl:id>
        <rdfs:label>Tongomainge</rdfs:label>
    </owl:NamedIndividual>
    


    <!-- http://purl.obolibrary.org/obo/GAZ_00255839 -->

    <owl:NamedIndividual rdf:about="http://purl.obolibrary.org/obo/GAZ_00255839">
        <rdf:type rdf:resource="http://purl.obolibrary.org/obo/ENVO_00000856"/>
        <obo:RO_0001025 rdf:resource="http://purl.obolibrary.org/obo/GAZ_00016929"/>
        <obo:IAO_0000115>A populated place. A village.</obo:IAO_0000115>
        <oboInOwl:hasOBONamespace>GAZ</oboInOwl:hasOBONamespace>
        <oboInOwl:id>GAZ:00255839</oboInOwl:id>
        <rdfs:label>Ngotokanaba</rdfs:label>
    </owl:NamedIndividual>
    


    <!-- http://purl.obolibrary.org/obo/GAZ_00255840 -->

    <owl:NamedIndividual rdf:about="http://purl.obolibrary.org/obo/GAZ_00255840">
        <rdf:type rdf:resource="http://purl.obolibrary.org/obo/ENVO_00000856"/>
        <obo:RO_0001025 rdf:resource="http://purl.obolibrary.org/obo/GAZ_00016929"/>
        <obo:IAO_0000115>A populated place. A village.</obo:IAO_0000115>
        <oboInOwl:hasOBONamespace>GAZ</oboInOwl:hasOBONamespace>
        <oboInOwl:id>GAZ:00255840</oboInOwl:id>
        <rdfs:label>Pauta</rdfs:label>
    </owl:NamedIndividual>
    


    <!-- http://purl.obolibrary.org/obo/GAZ_00255841 -->

    <owl:NamedIndividual rdf:about="http://purl.obolibrary.org/obo/GAZ_00255841">
        <rdf:type rdf:resource="http://purl.obolibrary.org/obo/ENVO_00000856"/>
        <obo:RO_0001025 rdf:resource="http://purl.obolibrary.org/obo/GAZ_00016929"/>
        <obo:IAO_0000115>A populated place. A village.</obo:IAO_0000115>
        <oboInOwl:hasOBONamespace>GAZ</oboInOwl:hasOBONamespace>
        <oboInOwl:id>GAZ:00255841</oboInOwl:id>
        <rdfs:label>Ngongona</rdfs:label>
    </owl:NamedIndividual>
    


    <!-- http://purl.obolibrary.org/obo/GAZ_00255842 -->

    <owl:NamedIndividual rdf:about="http://purl.obolibrary.org/obo/GAZ_00255842">
        <rdf:type rdf:resource="http://purl.obolibrary.org/obo/ENVO_00000856"/>
        <obo:RO_0001025 rdf:resource="http://purl.obolibrary.org/obo/GAZ_00016929"/>
        <obo:IAO_0000115>A populated place. A village.</obo:IAO_0000115>
        <oboInOwl:hasOBONamespace>GAZ</oboInOwl:hasOBONamespace>
        <oboInOwl:id>GAZ:00255842</oboInOwl:id>
        <rdfs:label>Gongau</rdfs:label>
    </owl:NamedIndividual>
    


    <!-- http://purl.obolibrary.org/obo/GAZ_00255843 -->

    <owl:NamedIndividual rdf:about="http://purl.obolibrary.org/obo/GAZ_00255843">
        <rdf:type rdf:resource="http://purl.obolibrary.org/obo/ENVO_00000856"/>
        <obo:RO_0001025 rdf:resource="http://purl.obolibrary.org/obo/GAZ_00016929"/>
        <obo:IAO_0000115>A populated place. A village.</obo:IAO_0000115>
        <oboInOwl:hasOBONamespace>GAZ</oboInOwl:hasOBONamespace>
        <oboInOwl:id>GAZ:00255843</oboInOwl:id>
        <rdfs:label>Ahenoa</rdfs:label>
    </owl:NamedIndividual>
    


    <!-- http://purl.obolibrary.org/obo/GAZ_00255844 -->

    <owl:NamedIndividual rdf:about="http://purl.obolibrary.org/obo/GAZ_00255844">
        <rdf:type rdf:resource="http://purl.obolibrary.org/obo/ENVO_00000856"/>
        <obo:RO_0001025 rdf:resource="http://purl.obolibrary.org/obo/GAZ_00016929"/>
        <obo:IAO_0000115>A populated place. A village.</obo:IAO_0000115>
        <oboInOwl:hasOBONamespace>GAZ</oboInOwl:hasOBONamespace>
        <oboInOwl:id>GAZ:00255844</oboInOwl:id>
        <rdfs:label>Matangi</rdfs:label>
    </owl:NamedIndividual>
    


    <!-- http://purl.obolibrary.org/obo/GAZ_00255845 -->

    <owl:NamedIndividual rdf:about="http://purl.obolibrary.org/obo/GAZ_00255845">
        <rdf:type rdf:resource="http://purl.obolibrary.org/obo/ENVO_00000856"/>
        <obo:RO_0001025 rdf:resource="http://purl.obolibrary.org/obo/GAZ_00016929"/>
        <obo:IAO_0000115>A populated place. A village.</obo:IAO_0000115>
        <oboInOwl:hasOBONamespace>GAZ</oboInOwl:hasOBONamespace>
        <oboInOwl:id>GAZ:00255845</oboInOwl:id>
        <rdfs:label>NukuTonga</rdfs:label>
    </owl:NamedIndividual>
    


    <!-- http://purl.obolibrary.org/obo/GAZ_00255846 -->

    <owl:NamedIndividual rdf:about="http://purl.obolibrary.org/obo/GAZ_00255846">
        <rdf:type rdf:resource="http://purl.obolibrary.org/obo/ENVO_00000856"/>
        <obo:RO_0001025 rdf:resource="http://purl.obolibrary.org/obo/GAZ_00001170"/>
        <obo:IAO_0000115>A populated place. A village.</obo:IAO_0000115>
        <oboInOwl:hasOBONamespace>GAZ</oboInOwl:hasOBONamespace>
        <oboInOwl:id>GAZ:00255846</oboInOwl:id>
        <rdfs:label>Mua</rdfs:label>
    </owl:NamedIndividual>
    


    <!-- http://purl.obolibrary.org/obo/GAZ_00255847 -->

    <owl:NamedIndividual rdf:about="http://purl.obolibrary.org/obo/GAZ_00255847">
        <rdf:type rdf:resource="http://purl.obolibrary.org/obo/ENVO_00000856"/>
        <obo:RO_0001025 rdf:resource="http://purl.obolibrary.org/obo/GAZ_00001170"/>
        <obo:IAO_0000115>A populated place. A village.</obo:IAO_0000115>
        <oboInOwl:hasOBONamespace>GAZ</oboInOwl:hasOBONamespace>
        <oboInOwl:id>GAZ:00255847</oboInOwl:id>
        <rdfs:label>Muri</rdfs:label>
    </owl:NamedIndividual>
    


    <!-- http://purl.obolibrary.org/obo/GAZ_00255848 -->

    <owl:NamedIndividual rdf:about="http://purl.obolibrary.org/obo/GAZ_00255848">
        <obo:RO_0001025 rdf:resource="http://purl.obolibrary.org/obo/GAZ_00009557"/>
        <obo:IAO_0000115>An island in the Solomon Islands; it is located in Temotu Province.</obo:IAO_0000115>
        <oboInOwl:hasOBONamespace>GAZ</oboInOwl:hasOBONamespace>
        <oboInOwl:id>GAZ:00255848</oboInOwl:id>
        <rdfs:label>Lomlom Island</rdfs:label>
    </owl:NamedIndividual>
    


    <!-- http://purl.obolibrary.org/obo/GAZ_00255849 -->

    <owl:NamedIndividual rdf:about="http://purl.obolibrary.org/obo/GAZ_00255849">
        <rdf:type rdf:resource="http://purl.obolibrary.org/obo/ENVO_00000856"/>
        <obo:RO_0001025 rdf:resource="http://purl.obolibrary.org/obo/GAZ_00016957"/>
        <obo:IAO_0000115>A populated place. A village.</obo:IAO_0000115>
        <oboInOwl:hasOBONamespace>GAZ</oboInOwl:hasOBONamespace>
        <oboInOwl:id>GAZ:00255849</oboInOwl:id>
        <rdfs:label>Tuo</rdfs:label>
    </owl:NamedIndividual>
    


    <!-- http://purl.obolibrary.org/obo/GAZ_00255850 -->

    <owl:NamedIndividual rdf:about="http://purl.obolibrary.org/obo/GAZ_00255850">
        <rdf:type rdf:resource="http://purl.obolibrary.org/obo/ENVO_00000856"/>
        <obo:RO_0001025 rdf:resource="http://purl.obolibrary.org/obo/GAZ_00016957"/>
        <obo:IAO_0000115>A populated place. A village.</obo:IAO_0000115>
        <oboInOwl:hasOBONamespace>GAZ</oboInOwl:hasOBONamespace>
        <oboInOwl:id>GAZ:00255850</oboInOwl:id>
        <rdfs:label>Maluba</rdfs:label>
    </owl:NamedIndividual>
    


    <!-- http://purl.obolibrary.org/obo/GAZ_00255851 -->

    <owl:NamedIndividual rdf:about="http://purl.obolibrary.org/obo/GAZ_00255851">
        <rdf:type rdf:resource="http://purl.obolibrary.org/obo/ENVO_00000856"/>
        <obo:RO_0001025 rdf:resource="http://purl.obolibrary.org/obo/GAZ_00016957"/>
        <obo:IAO_0000115>A populated place. A village.</obo:IAO_0000115>
        <oboInOwl:hasOBONamespace>GAZ</oboInOwl:hasOBONamespace>
        <oboInOwl:id>GAZ:00255851</oboInOwl:id>
        <rdfs:label>Tanga</rdfs:label>
    </owl:NamedIndividual>
    


    <!-- http://purl.obolibrary.org/obo/GAZ_00255852 -->

    <owl:NamedIndividual rdf:about="http://purl.obolibrary.org/obo/GAZ_00255852">
        <rdf:type rdf:resource="http://purl.obolibrary.org/obo/ENVO_00000856"/>
        <obo:RO_0001025 rdf:resource="http://purl.obolibrary.org/obo/GAZ_00016957"/>
        <obo:IAO_0000115>A populated place. A village.</obo:IAO_0000115>
        <oboInOwl:hasOBONamespace>GAZ</oboInOwl:hasOBONamespace>
        <oboInOwl:id>GAZ:00255852</oboInOwl:id>
        <rdfs:label>Malapu</rdfs:label>
    </owl:NamedIndividual>
    


    <!-- http://purl.obolibrary.org/obo/GAZ_00255853 -->

    <owl:NamedIndividual rdf:about="http://purl.obolibrary.org/obo/GAZ_00255853">
        <obo:RO_0001025 rdf:resource="http://purl.obolibrary.org/obo/GAZ_00016938"/>
        <obo:IAO_0000115>A populated place. The provincial capital of Temotu Province, Solomon Islands.</obo:IAO_0000115>
        <oboInOwl:hasOBONamespace>GAZ</oboInOwl:hasOBONamespace>
        <oboInOwl:id>GAZ:00255853</oboInOwl:id>
        <rdfs:label>Lata</rdfs:label>
    </owl:NamedIndividual>
    


    <!-- http://purl.obolibrary.org/obo/GAZ_00255854 -->

    <owl:NamedIndividual rdf:about="http://purl.obolibrary.org/obo/GAZ_00255854">
        <obo:RO_0001025 rdf:resource="http://purl.obolibrary.org/obo/GAZ_00007211"/>
        <obo:IAO_0000115>A crater lake.</obo:IAO_0000115>
        <oboInOwl:hasOBONamespace>GAZ</oboInOwl:hasOBONamespace>
        <oboInOwl:id>GAZ:00255854</oboInOwl:id>
        <rdfs:label>Te Roto</rdfs:label>
    </owl:NamedIndividual>
    


    <!-- http://purl.obolibrary.org/obo/GAZ_00255855 -->

    <owl:NamedIndividual rdf:about="http://purl.obolibrary.org/obo/GAZ_00255855">
        <rdf:type rdf:resource="http://purl.obolibrary.org/obo/ENVO_00000856"/>
        <obo:RO_0001025 rdf:resource="http://purl.obolibrary.org/obo/GAZ_00007211"/>
        <obo:IAO_0000115>A populated place. A village.</obo:IAO_0000115>
        <oboInOwl:hasOBONamespace>GAZ</oboInOwl:hasOBONamespace>
        <oboInOwl:id>GAZ:00255855</oboInOwl:id>
        <rdfs:label>Matautu</rdfs:label>
    </owl:NamedIndividual>
    


    <!-- http://purl.obolibrary.org/obo/GAZ_00255856 -->

    <owl:NamedIndividual rdf:about="http://purl.obolibrary.org/obo/GAZ_00255856">
        <rdf:type rdf:resource="http://purl.obolibrary.org/obo/ENVO_00000856"/>
        <obo:RO_0001025 rdf:resource="http://purl.obolibrary.org/obo/GAZ_00016933"/>
        <obo:IAO_0000115>A populated place. A village.</obo:IAO_0000115>
        <oboInOwl:hasOBONamespace>GAZ</oboInOwl:hasOBONamespace>
        <oboInOwl:id>GAZ:00255856</oboInOwl:id>
        <rdfs:label>Avita</rdfs:label>
    </owl:NamedIndividual>
    


    <!-- http://purl.obolibrary.org/obo/GAZ_00255857 -->

    <owl:NamedIndividual rdf:about="http://purl.obolibrary.org/obo/GAZ_00255857">
        <rdf:type rdf:resource="http://purl.obolibrary.org/obo/ENVO_00000856"/>
        <obo:RO_0001025 rdf:resource="http://purl.obolibrary.org/obo/GAZ_00016933"/>
        <obo:IAO_0000115>A populated place. A village.</obo:IAO_0000115>
        <oboInOwl:hasOBONamespace>GAZ</oboInOwl:hasOBONamespace>
        <oboInOwl:id>GAZ:00255857</oboInOwl:id>
        <rdfs:label>Malombo</rdfs:label>
    </owl:NamedIndividual>
    


    <!-- http://purl.obolibrary.org/obo/GAZ_00255858 -->

    <owl:NamedIndividual rdf:about="http://purl.obolibrary.org/obo/GAZ_00255858">
        <rdf:type rdf:resource="http://purl.obolibrary.org/obo/ENVO_00000856"/>
        <obo:RO_0001025 rdf:resource="http://purl.obolibrary.org/obo/GAZ_00016933"/>
        <obo:IAO_0000115>A populated place. A village.</obo:IAO_0000115>
        <oboInOwl:hasOBONamespace>GAZ</oboInOwl:hasOBONamespace>
        <oboInOwl:id>GAZ:00255858</oboInOwl:id>
        <rdfs:label>Tanimbili</rdfs:label>
    </owl:NamedIndividual>
    


    <!-- http://purl.obolibrary.org/obo/GAZ_00255859 -->

    <owl:NamedIndividual rdf:about="http://purl.obolibrary.org/obo/GAZ_00255859">
        <rdf:type rdf:resource="http://purl.obolibrary.org/obo/ENVO_00000856"/>
        <obo:RO_0001025 rdf:resource="http://purl.obolibrary.org/obo/GAZ_00016933"/>
        <obo:IAO_0000115>A populated place. A village.</obo:IAO_0000115>
        <oboInOwl:hasOBONamespace>GAZ</oboInOwl:hasOBONamespace>
        <oboInOwl:id>GAZ:00255859</oboInOwl:id>
        <rdfs:label>Apakho</rdfs:label>
    </owl:NamedIndividual>
    


    <!-- http://purl.obolibrary.org/obo/GAZ_00255860 -->

    <owl:NamedIndividual rdf:about="http://purl.obolibrary.org/obo/GAZ_00255860">
        <rdf:type rdf:resource="http://purl.obolibrary.org/obo/ENVO_00000856"/>
        <obo:RO_0001025 rdf:resource="http://purl.obolibrary.org/obo/GAZ_00016933"/>
        <obo:IAO_0000115>A populated place. A village.</obo:IAO_0000115>
        <oboInOwl:hasOBONamespace>GAZ</oboInOwl:hasOBONamespace>
        <oboInOwl:id>GAZ:00255860</oboInOwl:id>
        <rdfs:label>Nembao</rdfs:label>
    </owl:NamedIndividual>
    


    <!-- http://purl.obolibrary.org/obo/GAZ_00255861 -->

    <owl:NamedIndividual rdf:about="http://purl.obolibrary.org/obo/GAZ_00255861">
        <obo:RO_0001025 rdf:resource="http://purl.obolibrary.org/obo/GAZ_00016932"/>
        <obo:IAO_0000115>An island.</obo:IAO_0000115>
        <oboInOwl:hasOBONamespace>GAZ</oboInOwl:hasOBONamespace>
        <oboInOwl:id>GAZ:00255861</oboInOwl:id>
        <rdfs:label>Manieve Island</rdfs:label>
    </owl:NamedIndividual>
    


    <!-- http://purl.obolibrary.org/obo/GAZ_00255862 -->

    <owl:NamedIndividual rdf:about="http://purl.obolibrary.org/obo/GAZ_00255862">
        <obo:RO_0001025 rdf:resource="http://purl.obolibrary.org/obo/GAZ_00016932"/>
        <obo:IAO_0000115>An island.</obo:IAO_0000115>
        <oboInOwl:hasOBONamespace>GAZ</oboInOwl:hasOBONamespace>
        <oboInOwl:id>GAZ:00255862</oboInOwl:id>
        <rdfs:label>Nomianu Island</rdfs:label>
    </owl:NamedIndividual>
    


    <!-- http://purl.obolibrary.org/obo/GAZ_00255863 -->

    <owl:NamedIndividual rdf:about="http://purl.obolibrary.org/obo/GAZ_00255863">
        <obo:RO_0001025 rdf:resource="http://purl.obolibrary.org/obo/GAZ_00016932"/>
        <obo:IAO_0000115>An island.</obo:IAO_0000115>
        <oboInOwl:hasOBONamespace>GAZ</oboInOwl:hasOBONamespace>
        <oboInOwl:id>GAZ:00255863</oboInOwl:id>
        <rdfs:label>Nanunga Island</rdfs:label>
    </owl:NamedIndividual>
    


    <!-- http://purl.obolibrary.org/obo/GAZ_00255864 -->

    <owl:NamedIndividual rdf:about="http://purl.obolibrary.org/obo/GAZ_00255864">
        <obo:RO_0001025 rdf:resource="http://purl.obolibrary.org/obo/GAZ_00016889"/>
        <obo:IAO_0000115>A natural harbour between Mono and Stirling Islands of the Treasury Islands, Solomon Islands.</obo:IAO_0000115>
        <oboInOwl:hasOBONamespace>GAZ</oboInOwl:hasOBONamespace>
        <oboInOwl:id>GAZ:00255864</oboInOwl:id>
        <rdfs:label>Blanche Harbor</rdfs:label>
    </owl:NamedIndividual>
    


    <!-- http://purl.obolibrary.org/obo/GAZ_00255865 -->

    <owl:NamedIndividual rdf:about="http://purl.obolibrary.org/obo/GAZ_00255865">
        <obo:RO_0001025 rdf:resource="http://purl.obolibrary.org/obo/GAZ_00009132"/>
        <obo:IAO_0000115>The largest island of the Shortland Islands, Solomon Islands.</obo:IAO_0000115>
        <oboInOwl:hasOBONamespace>GAZ</oboInOwl:hasOBONamespace>
        <oboInOwl:id>GAZ:00255865</oboInOwl:id>
        <rdfs:label>Shortland Island</rdfs:label>
    </owl:NamedIndividual>
    


    <!-- http://purl.obolibrary.org/obo/GAZ_00255866 -->

    <owl:NamedIndividual rdf:about="http://purl.obolibrary.org/obo/GAZ_00255866">
        <obo:RO_0001025 rdf:resource="http://purl.obolibrary.org/obo/GAZ_00009132"/>
        <obo:IAO_0000115>An island of the Shortland Islands Group in the Western Province of the Solomon Islands.</obo:IAO_0000115>
        <oboInOwl:hasOBONamespace>GAZ</oboInOwl:hasOBONamespace>
        <oboInOwl:id>GAZ:00255866</oboInOwl:id>
        <rdfs:label>Balalae Island</rdfs:label>
    </owl:NamedIndividual>
    


    <!-- http://purl.obolibrary.org/obo/GAZ_00255867 -->

    <owl:NamedIndividual rdf:about="http://purl.obolibrary.org/obo/GAZ_00255867">
        <rdf:type rdf:resource="http://purl.obolibrary.org/obo/ENVO_00000098"/>
        <obo:RO_0001025 rdf:resource="http://purl.obolibrary.org/obo/GAZ_00009133"/>
        <obo:IAO_0000115>An island in the Solomon Islands; it is located in the Western Province. A barrier island of the Marovo Lagoon.</obo:IAO_0000115>
        <oboInOwl:hasOBONamespace>GAZ</oboInOwl:hasOBONamespace>
        <oboInOwl:id>GAZ:00255867</oboInOwl:id>
        <rdfs:label>Uepi Island</rdfs:label>
    </owl:NamedIndividual>
    


    <!-- http://purl.obolibrary.org/obo/GAZ_00255868 -->

    <owl:NamedIndividual rdf:about="http://purl.obolibrary.org/obo/GAZ_00255868">
        <obo:RO_0001025 rdf:resource="http://purl.obolibrary.org/obo/GAZ_00012781"/>
        <obo:IAO_0000115>An island in the Solomon Islands; it is located in the Western Province.</obo:IAO_0000115>
        <oboInOwl:hasOBONamespace>GAZ</oboInOwl:hasOBONamespace>
        <oboInOwl:id>GAZ:00255868</oboInOwl:id>
        <rdfs:label>Telina Island</rdfs:label>
    </owl:NamedIndividual>
    


    <!-- http://purl.obolibrary.org/obo/GAZ_00255869 -->

    <owl:NamedIndividual rdf:about="http://purl.obolibrary.org/obo/GAZ_00255869">
        <obo:RO_0001025 rdf:resource="http://purl.obolibrary.org/obo/GAZ_00016895"/>
        <obo:IAO_0000115>A populated place.</obo:IAO_0000115>
        <oboInOwl:hasOBONamespace>GAZ</oboInOwl:hasOBONamespace>
        <oboInOwl:id>GAZ:00255869</oboInOwl:id>
        <rdfs:label>Baniata</rdfs:label>
    </owl:NamedIndividual>
    


    <!-- http://purl.obolibrary.org/obo/GAZ_00255870 -->

    <owl:NamedIndividual rdf:about="http://purl.obolibrary.org/obo/GAZ_00255870">
        <obo:RO_0001025 rdf:resource="http://purl.obolibrary.org/obo/GAZ_00016895"/>
        <obo:IAO_0000115>A populated place.</obo:IAO_0000115>
        <oboInOwl:hasOBONamespace>GAZ</oboInOwl:hasOBONamespace>
        <oboInOwl:id>GAZ:00255870</oboInOwl:id>
        <rdfs:label>Havilla</rdfs:label>
    </owl:NamedIndividual>
    


    <!-- http://purl.obolibrary.org/obo/GAZ_00255871 -->

    <owl:NamedIndividual rdf:about="http://purl.obolibrary.org/obo/GAZ_00255871">
        <obo:RO_0001025 rdf:resource="http://purl.obolibrary.org/obo/GAZ_00016895"/>
        <obo:IAO_0000115>A populated place.</obo:IAO_0000115>
        <oboInOwl:hasOBONamespace>GAZ</oboInOwl:hasOBONamespace>
        <oboInOwl:id>GAZ:00255871</oboInOwl:id>
        <rdfs:label>Retavo</rdfs:label>
    </owl:NamedIndividual>
    


    <!-- http://purl.obolibrary.org/obo/GAZ_00255872 -->

    <owl:NamedIndividual rdf:about="http://purl.obolibrary.org/obo/GAZ_00255872">
        <obo:RO_0001025 rdf:resource="http://purl.obolibrary.org/obo/GAZ_00016904"/>
        <obo:IAO_0000115>A populated place.</obo:IAO_0000115>
        <oboInOwl:hasOBONamespace>GAZ</oboInOwl:hasOBONamespace>
        <oboInOwl:id>GAZ:00255872</oboInOwl:id>
        <rdfs:label>Pienuna</rdfs:label>
    </owl:NamedIndividual>
    


    <!-- http://purl.obolibrary.org/obo/GAZ_00255873 -->

    <owl:NamedIndividual rdf:about="http://purl.obolibrary.org/obo/GAZ_00255873">
        <obo:RO_0001025 rdf:resource="http://purl.obolibrary.org/obo/GAZ_00016895"/>
        <obo:IAO_0000115>A populated place.</obo:IAO_0000115>
        <oboInOwl:hasOBONamespace>GAZ</oboInOwl:hasOBONamespace>
        <oboInOwl:id>GAZ:00255873</oboInOwl:id>
        <rdfs:label>Au</rdfs:label>
    </owl:NamedIndividual>
    


    <!-- http://purl.obolibrary.org/obo/GAZ_00255874 -->

    <owl:NamedIndividual rdf:about="http://purl.obolibrary.org/obo/GAZ_00255874">
        <obo:RO_0001025 rdf:resource="http://purl.obolibrary.org/obo/GAZ_00016895"/>
        <obo:IAO_0000115>A populated place.</obo:IAO_0000115>
        <oboInOwl:hasOBONamespace>GAZ</oboInOwl:hasOBONamespace>
        <oboInOwl:id>GAZ:00255874</oboInOwl:id>
        <rdfs:label>Vanikuva</rdfs:label>
    </owl:NamedIndividual>
    


    <!-- http://purl.obolibrary.org/obo/GAZ_00255875 -->

    <owl:NamedIndividual rdf:about="http://purl.obolibrary.org/obo/GAZ_00255875">
        <obo:RO_0001025 rdf:resource="http://purl.obolibrary.org/obo/GAZ_00016895"/>
        <obo:IAO_0000115>A populated place.</obo:IAO_0000115>
        <oboInOwl:hasOBONamespace>GAZ</oboInOwl:hasOBONamespace>
        <oboInOwl:id>GAZ:00255875</oboInOwl:id>
        <rdfs:label>Eghelo</rdfs:label>
    </owl:NamedIndividual>
    


    <!-- http://purl.obolibrary.org/obo/GAZ_00255876 -->

    <owl:NamedIndividual rdf:about="http://purl.obolibrary.org/obo/GAZ_00255876">
        <obo:RO_0001025 rdf:resource="http://purl.obolibrary.org/obo/GAZ_00016895"/>
        <obo:IAO_0000115>A populated place.</obo:IAO_0000115>
        <oboInOwl:hasOBONamespace>GAZ</oboInOwl:hasOBONamespace>
        <oboInOwl:id>GAZ:00255876</oboInOwl:id>
        <rdfs:label>Mburuku</rdfs:label>
    </owl:NamedIndividual>
    


    <!-- http://purl.obolibrary.org/obo/GAZ_00255877 -->

    <owl:NamedIndividual rdf:about="http://purl.obolibrary.org/obo/GAZ_00255877">
        <obo:RO_0001025 rdf:resource="http://purl.obolibrary.org/obo/GAZ_00016903"/>
        <obo:IAO_0000115>A populated place.</obo:IAO_0000115>
        <oboInOwl:hasOBONamespace>GAZ</oboInOwl:hasOBONamespace>
        <oboInOwl:id>GAZ:00255877</oboInOwl:id>
        <rdfs:label>Kumbolia</rdfs:label>
    </owl:NamedIndividual>
    


    <!-- http://purl.obolibrary.org/obo/GAZ_00255878 -->

    <owl:NamedIndividual rdf:about="http://purl.obolibrary.org/obo/GAZ_00255878">
        <obo:RO_0001025 rdf:resource="http://purl.obolibrary.org/obo/GAZ_00016903"/>
        <obo:IAO_0000115>A populated place.</obo:IAO_0000115>
        <oboInOwl:hasOBONamespace>GAZ</oboInOwl:hasOBONamespace>
        <oboInOwl:id>GAZ:00255878</oboInOwl:id>
        <rdfs:label>Mbilua</rdfs:label>
    </owl:NamedIndividual>
    


    <!-- http://purl.obolibrary.org/obo/GAZ_00255879 -->

    <owl:NamedIndividual rdf:about="http://purl.obolibrary.org/obo/GAZ_00255879">
        <obo:RO_0001025 rdf:resource="http://purl.obolibrary.org/obo/GAZ_00016903"/>
        <obo:IAO_0000115>A populated place.</obo:IAO_0000115>
        <oboInOwl:hasOBONamespace>GAZ</oboInOwl:hasOBONamespace>
        <oboInOwl:id>GAZ:00255879</oboInOwl:id>
        <rdfs:label>Mbarakoma</rdfs:label>
    </owl:NamedIndividual>
    


    <!-- http://purl.obolibrary.org/obo/GAZ_00255880 -->

    <owl:NamedIndividual rdf:about="http://purl.obolibrary.org/obo/GAZ_00255880">
        <obo:RO_0001025 rdf:resource="http://purl.obolibrary.org/obo/GAZ_00016894"/>
        <obo:IAO_0000115>A populated place.</obo:IAO_0000115>
        <oboInOwl:hasOBONamespace>GAZ</oboInOwl:hasOBONamespace>
        <oboInOwl:id>GAZ:00255880</oboInOwl:id>
        <rdfs:label>Nineveh</rdfs:label>
    </owl:NamedIndividual>
    


    <!-- http://purl.obolibrary.org/obo/GAZ_00255881 -->

    <owl:NamedIndividual rdf:about="http://purl.obolibrary.org/obo/GAZ_00255881">
        <obo:RO_0001025 rdf:resource="http://purl.obolibrary.org/obo/GAZ_00016894"/>
        <obo:IAO_0000115>A populated place.</obo:IAO_0000115>
        <oboInOwl:hasOBONamespace>GAZ</oboInOwl:hasOBONamespace>
        <oboInOwl:id>GAZ:00255881</oboInOwl:id>
        <rdfs:label>Saira</rdfs:label>
    </owl:NamedIndividual>
    


    <!-- http://purl.obolibrary.org/obo/GAZ_00255882 -->

    <owl:NamedIndividual rdf:about="http://purl.obolibrary.org/obo/GAZ_00255882">
        <rdf:type rdf:resource="http://purl.obolibrary.org/obo/ENVO_00000029"/>
        <obo:RO_0001025 rdf:resource="http://purl.obolibrary.org/obo/GAZ_00012781"/>
        <obo:IAO_0000115>A waterway in the Western Province of the Solomon Islands. It lies between the islands of Vella Lavella to the northwest, Kolombangara to the southeast, and Ghizo to the south. It connects New Georgia Sound to the northeast with the Solomon Sea to the south.</obo:IAO_0000115>
        <oboInOwl:hasOBONamespace>GAZ</oboInOwl:hasOBONamespace>
        <oboInOwl:id>GAZ:00255882</oboInOwl:id>
        <rdfs:label>Vella Gulf</rdfs:label>
    </owl:NamedIndividual>
    


    <!-- http://purl.obolibrary.org/obo/GAZ_00255884 -->

    <owl:NamedIndividual rdf:about="http://purl.obolibrary.org/obo/GAZ_00255884">
        <rdf:type rdf:resource="http://purl.obolibrary.org/obo/ENVO_00000029"/>
        <obo:RO_0001025 rdf:resource="http://purl.obolibrary.org/obo/GAZ_00012781"/>
        <obo:IAO_0000115>A waterway. It lies between the islands of Kolombangara to the west, Arundel Island (Kohinggo) to the southwest, and New Georgia to the south and east. To the north, it opens into New Georgia Sound. To the southwest, it connects via Blackett Strait to Vella Gulf and the Solomon Sea.</obo:IAO_0000115>
        <oboInOwl:hasOBONamespace>GAZ</oboInOwl:hasOBONamespace>
        <oboInOwl:id>GAZ:00255884</oboInOwl:id>
        <rdfs:label>Kula Gulf</rdfs:label>
    </owl:NamedIndividual>
    


    <!-- http://purl.obolibrary.org/obo/GAZ_00255885 -->

    <owl:NamedIndividual rdf:about="http://purl.obolibrary.org/obo/GAZ_00255885">
        <obo:RO_0001025 rdf:resource="http://purl.obolibrary.org/obo/GAZ_00012781"/>
        <obo:IAO_0000115>A waterway in the Western Province of the Solomon Islands. It lies between the islands of New Georgia and Vangunu to the northeast, and Rendova and Tetepare to the southwest. It connects to the Solomon Sea at both east and west ends.</obo:IAO_0000115>
        <oboInOwl:hasOBONamespace>GAZ</oboInOwl:hasOBONamespace>
        <oboInOwl:id>GAZ:00255885</oboInOwl:id>
        <rdfs:label>Blanche Channel</rdfs:label>
    </owl:NamedIndividual>
    


    <!-- http://purl.obolibrary.org/obo/GAZ_00255886 -->

    <owl:NamedIndividual rdf:about="http://purl.obolibrary.org/obo/GAZ_00255886">
        <obo:RO_0001025 rdf:resource="http://purl.obolibrary.org/obo/GAZ_00012781"/>
        <obo:IAO_0000115>An island.</obo:IAO_0000115>
        <oboInOwl:hasOBONamespace>GAZ</oboInOwl:hasOBONamespace>
        <oboInOwl:id>GAZ:00255886</oboInOwl:id>
        <rdfs:label>Nusatupe Island</rdfs:label>
    </owl:NamedIndividual>
    


    <!-- http://purl.obolibrary.org/obo/GAZ_00255887 -->

    <owl:NamedIndividual rdf:about="http://purl.obolibrary.org/obo/GAZ_00255887">
        <obo:RO_0001025 rdf:resource="http://purl.obolibrary.org/obo/GAZ_00012781"/>
        <obo:IAO_0000115>An island.</obo:IAO_0000115>
        <oboInOwl:hasOBONamespace>GAZ</oboInOwl:hasOBONamespace>
        <oboInOwl:id>GAZ:00255887</oboInOwl:id>
        <rdfs:label>Nakaza Island</rdfs:label>
    </owl:NamedIndividual>
    


    <!-- http://purl.obolibrary.org/obo/GAZ_00255888 -->

    <owl:NamedIndividual rdf:about="http://purl.obolibrary.org/obo/GAZ_00255888">
        <obo:RO_0001025 rdf:resource="http://purl.obolibrary.org/obo/GAZ_00012781"/>
        <obo:IAO_0000115>An island.</obo:IAO_0000115>
        <oboInOwl:hasOBONamespace>GAZ</oboInOwl:hasOBONamespace>
        <oboInOwl:id>GAZ:00255888</oboInOwl:id>
        <rdfs:label>Mondomondo Island</rdfs:label>
    </owl:NamedIndividual>
    


    <!-- http://purl.obolibrary.org/obo/GAZ_00255889 -->

    <owl:NamedIndividual rdf:about="http://purl.obolibrary.org/obo/GAZ_00255889">
        <rdf:type rdf:resource="http://purl.obolibrary.org/obo/ENVO_00000222"/>
        <obo:RO_0001025 rdf:resource="http://purl.obolibrary.org/obo/GAZ_00009133"/>
        <obo:IAO_0000115>A volcanic island. Located in the eastern part of the New Georgia Islands.</obo:IAO_0000115>
        <oboInOwl:hasOBONamespace>GAZ</oboInOwl:hasOBONamespace>
        <oboInOwl:id>GAZ:00255889</oboInOwl:id>
        <rdfs:label>Mbulo Island</rdfs:label>
    </owl:NamedIndividual>
    


    <!-- http://purl.obolibrary.org/obo/GAZ_00255890 -->

    <owl:NamedIndividual rdf:about="http://purl.obolibrary.org/obo/GAZ_00255890">
        <obo:RO_0001025 rdf:resource="http://purl.obolibrary.org/obo/GAZ_00016902"/>
        <obo:IAO_0000115>A populated place. The capital of the Western Province in the Solomon Islands.</obo:IAO_0000115>
        <oboInOwl:hasOBONamespace>GAZ</oboInOwl:hasOBONamespace>
        <oboInOwl:id>GAZ:00255890</oboInOwl:id>
        <rdfs:label>Gizo</rdfs:label>
    </owl:NamedIndividual>
    


    <!-- http://purl.obolibrary.org/obo/GAZ_00255891 -->

    <owl:NamedIndividual rdf:about="http://purl.obolibrary.org/obo/GAZ_00255891">
        <obo:RO_0001025 rdf:resource="http://purl.obolibrary.org/obo/GAZ_00012781"/>
        <obo:IAO_0000115>An island in the Solomon Islands; it is located in the Western Province.</obo:IAO_0000115>
        <oboInOwl:hasOBONamespace>GAZ</oboInOwl:hasOBONamespace>
        <oboInOwl:id>GAZ:00255891</oboInOwl:id>
        <rdfs:label>Matikuri Island</rdfs:label>
    </owl:NamedIndividual>
    


    <!-- http://purl.obolibrary.org/obo/GAZ_00255892 -->

    <owl:NamedIndividual rdf:about="http://purl.obolibrary.org/obo/GAZ_00255892">
        <obo:RO_0001025 rdf:resource="http://purl.obolibrary.org/obo/GAZ_00051763"/>
        <obo:IAO_0000115>An island in the Solomon Islands; it is located in the Western Province.</obo:IAO_0000115>
        <oboInOwl:hasOBONamespace>GAZ</oboInOwl:hasOBONamespace>
        <oboInOwl:id>GAZ:00255892</oboInOwl:id>
        <rdfs:label>Marovo Island</rdfs:label>
    </owl:NamedIndividual>
    


    <!-- http://purl.obolibrary.org/obo/GAZ_00255893 -->

    <owl:NamedIndividual rdf:about="http://purl.obolibrary.org/obo/GAZ_00255893">
        <obo:RO_0001025 rdf:resource="http://purl.obolibrary.org/obo/GAZ_00012781"/>
        <obo:IAO_0000115>An island in the Solomon Islands; it is located in the Western Province.</obo:IAO_0000115>
        <oboInOwl:hasOBONamespace>GAZ</oboInOwl:hasOBONamespace>
        <oboInOwl:id>GAZ:00255893</oboInOwl:id>
        <rdfs:label>Lola Island</rdfs:label>
    </owl:NamedIndividual>
    


    <!-- http://purl.obolibrary.org/obo/GAZ_00255894 -->

    <owl:NamedIndividual rdf:about="http://purl.obolibrary.org/obo/GAZ_00255894">
        <obo:RO_0001025 rdf:resource="http://purl.obolibrary.org/obo/GAZ_00012781"/>
        <obo:IAO_0000115>An island in the Solomon Islands; it is located in the Western Province.</obo:IAO_0000115>
        <oboInOwl:hasOBONamespace>GAZ</oboInOwl:hasOBONamespace>
        <oboInOwl:id>GAZ:00255894</oboInOwl:id>
        <rdfs:label>Logha Island</rdfs:label>
    </owl:NamedIndividual>
    


    <!-- http://purl.obolibrary.org/obo/GAZ_00255895 -->

    <owl:NamedIndividual rdf:about="http://purl.obolibrary.org/obo/GAZ_00255895">
        <obo:RO_0001025 rdf:resource="http://purl.obolibrary.org/obo/GAZ_00012781"/>
        <obo:IAO_0000115>An island in the Solomon Islands; it is located in the Western Province.</obo:IAO_0000115>
        <oboInOwl:hasOBONamespace>GAZ</oboInOwl:hasOBONamespace>
        <oboInOwl:id>GAZ:00255895</oboInOwl:id>
        <rdfs:label>Liapari Island</rdfs:label>
    </owl:NamedIndividual>
    


    <!-- http://purl.obolibrary.org/obo/GAZ_00255896 -->

    <owl:NamedIndividual rdf:about="http://purl.obolibrary.org/obo/GAZ_00255896">
        <obo:RO_0001025 rdf:resource="http://purl.obolibrary.org/obo/GAZ_00012781"/>
        <obo:IAO_0000115>An island in the Solomon Islands; it is located in the Western Province.</obo:IAO_0000115>
        <oboInOwl:hasOBONamespace>GAZ</oboInOwl:hasOBONamespace>
        <oboInOwl:id>GAZ:00255896</oboInOwl:id>
        <rdfs:label>Kingguru Island</rdfs:label>
    </owl:NamedIndividual>
    


    <!-- http://purl.obolibrary.org/obo/GAZ_00255897 -->

    <owl:NamedIndividual rdf:about="http://purl.obolibrary.org/obo/GAZ_00255897">
        <obo:RO_0001025 rdf:resource="http://purl.obolibrary.org/obo/GAZ_00012781"/>
        <obo:IAO_0000115>An island in the Solomon Islands; it is located in the Western Province.</obo:IAO_0000115>
        <oboInOwl:hasOBONamespace>GAZ</oboInOwl:hasOBONamespace>
        <oboInOwl:id>GAZ:00255897</oboInOwl:id>
        <rdfs:label>Kiambe Island</rdfs:label>
    </owl:NamedIndividual>
    


    <!-- http://purl.obolibrary.org/obo/GAZ_00255898 -->

    <owl:NamedIndividual rdf:about="http://purl.obolibrary.org/obo/GAZ_00255898">
        <obo:RO_0001025 rdf:resource="http://purl.obolibrary.org/obo/GAZ_00009133"/>
        <obo:IAO_0000115>An island.</obo:IAO_0000115>
        <oboInOwl:hasOBONamespace>GAZ</oboInOwl:hasOBONamespace>
        <oboInOwl:id>GAZ:00255898</oboInOwl:id>
        <rdfs:label>Kasolo Island</rdfs:label>
    </owl:NamedIndividual>
    


    <!-- http://purl.obolibrary.org/obo/GAZ_00255899 -->

    <owl:NamedIndividual rdf:about="http://purl.obolibrary.org/obo/GAZ_00255899">
        <obo:RO_0001025 rdf:resource="http://purl.obolibrary.org/obo/GAZ_00012781"/>
        <obo:IAO_0000115>An island in the Solomon Islands; it is located in the Western Province.</obo:IAO_0000115>
        <oboInOwl:hasOBONamespace>GAZ</oboInOwl:hasOBONamespace>
        <oboInOwl:id>GAZ:00255899</oboInOwl:id>
        <rdfs:label>Ghoi Island</rdfs:label>
    </owl:NamedIndividual>
    


    <!-- http://purl.obolibrary.org/obo/GAZ_00255900 -->

    <owl:NamedIndividual rdf:about="http://purl.obolibrary.org/obo/GAZ_00255900">
        <obo:RO_0001025 rdf:resource="http://purl.obolibrary.org/obo/GAZ_00012781"/>
        <obo:IAO_0000115>An island in the Solomon Islands, located in the Western Province.</obo:IAO_0000115>
        <oboInOwl:hasOBONamespace>GAZ</oboInOwl:hasOBONamespace>
        <oboInOwl:id>GAZ:00255900</oboInOwl:id>
        <rdfs:label>Faisi Island</rdfs:label>
    </owl:NamedIndividual>
    


    <!-- http://purl.obolibrary.org/obo/GAZ_00255901 -->

    <owl:NamedIndividual rdf:about="http://purl.obolibrary.org/obo/GAZ_00255901">
        <obo:RO_0001025 rdf:resource="http://purl.obolibrary.org/obo/GAZ_00009133"/>
        <obo:IAO_0000115>One of the Solomon Islands, near Rendova Island.</obo:IAO_0000115>
        <oboInOwl:hasOBONamespace>GAZ</oboInOwl:hasOBONamespace>
        <oboInOwl:id>GAZ:00255901</oboInOwl:id>
        <rdfs:label>Lumbari Island</rdfs:label>
    </owl:NamedIndividual>
    


    <!-- http://purl.obolibrary.org/obo/GAZ_00255902 -->

    <owl:NamedIndividual rdf:about="http://purl.obolibrary.org/obo/GAZ_00255902">
        <obo:RO_0001025 rdf:resource="http://purl.obolibrary.org/obo/GAZ_00016898"/>
        <obo:IAO_0000115>A populated place.</obo:IAO_0000115>
        <oboInOwl:hasOBONamespace>GAZ</oboInOwl:hasOBONamespace>
        <oboInOwl:id>GAZ:00255902</oboInOwl:id>
        <rdfs:label>Menakasapa</rdfs:label>
    </owl:NamedIndividual>
    


    <!-- http://purl.obolibrary.org/obo/GAZ_00255903 -->

    <owl:NamedIndividual rdf:about="http://purl.obolibrary.org/obo/GAZ_00255903">
        <obo:RO_0001025 rdf:resource="http://purl.obolibrary.org/obo/GAZ_00016898"/>
        <obo:IAO_0000115>A populated place.</obo:IAO_0000115>
        <oboInOwl:hasOBONamespace>GAZ</oboInOwl:hasOBONamespace>
        <oboInOwl:id>GAZ:00255903</oboInOwl:id>
        <rdfs:label>Hovoro</rdfs:label>
    </owl:NamedIndividual>
    


    <!-- http://purl.obolibrary.org/obo/GAZ_00255904 -->

    <owl:NamedIndividual rdf:about="http://purl.obolibrary.org/obo/GAZ_00255904">
        <obo:RO_0001025 rdf:resource="http://purl.obolibrary.org/obo/GAZ_00016898"/>
        <obo:IAO_0000115>A populated place.</obo:IAO_0000115>
        <oboInOwl:hasOBONamespace>GAZ</oboInOwl:hasOBONamespace>
        <oboInOwl:id>GAZ:00255904</oboInOwl:id>
        <rdfs:label>Hapai</rdfs:label>
    </owl:NamedIndividual>
    


    <!-- http://purl.obolibrary.org/obo/GAZ_00255905 -->

    <owl:NamedIndividual rdf:about="http://purl.obolibrary.org/obo/GAZ_00255905">
        <obo:RO_0001025 rdf:resource="http://purl.obolibrary.org/obo/GAZ_00016898"/>
        <obo:IAO_0000115>A populated place.</obo:IAO_0000115>
        <oboInOwl:hasOBONamespace>GAZ</oboInOwl:hasOBONamespace>
        <oboInOwl:id>GAZ:00255905</oboInOwl:id>
        <rdfs:label>Mbiula</rdfs:label>
    </owl:NamedIndividual>
    


    <!-- http://purl.obolibrary.org/obo/GAZ_00255906 -->

    <owl:NamedIndividual rdf:about="http://purl.obolibrary.org/obo/GAZ_00255906">
        <obo:RO_0001025 rdf:resource="http://purl.obolibrary.org/obo/GAZ_00016898"/>
        <obo:IAO_0000115>A populated place.</obo:IAO_0000115>
        <oboInOwl:hasOBONamespace>GAZ</oboInOwl:hasOBONamespace>
        <oboInOwl:id>GAZ:00255906</oboInOwl:id>
        <rdfs:label>Mbanga</rdfs:label>
    </owl:NamedIndividual>
    


    <!-- http://purl.obolibrary.org/obo/GAZ_00255907 -->

    <owl:NamedIndividual rdf:about="http://purl.obolibrary.org/obo/GAZ_00255907">
        <obo:RO_0001025 rdf:resource="http://purl.obolibrary.org/obo/GAZ_00016898"/>
        <obo:IAO_0000115>A populated place. The largest settlement on the island of New Georgia in the Western Province of the Solomon Islands.</obo:IAO_0000115>
        <oboInOwl:hasOBONamespace>GAZ</oboInOwl:hasOBONamespace>
        <oboInOwl:id>GAZ:00255907</oboInOwl:id>
        <rdfs:label>Munda</rdfs:label>
    </owl:NamedIndividual>
    


    <!-- http://purl.obolibrary.org/obo/GAZ_00255908 -->

    <owl:NamedIndividual rdf:about="http://purl.obolibrary.org/obo/GAZ_00255908">
        <obo:RO_0001025 rdf:resource="http://purl.obolibrary.org/obo/GAZ_00016898"/>
        <oboInOwl:hasOBONamespace>GAZ</oboInOwl:hasOBONamespace>
        <oboInOwl:id>GAZ:00255908</oboInOwl:id>
        <rdfs:label>Tetemara</rdfs:label>
    </owl:NamedIndividual>
    


    <!-- http://purl.obolibrary.org/obo/GAZ_00255909 -->

    <owl:NamedIndividual rdf:about="http://purl.obolibrary.org/obo/GAZ_00255909">
        <obo:RO_0001025 rdf:resource="http://purl.obolibrary.org/obo/GAZ_00016898"/>
        <oboInOwl:hasOBONamespace>GAZ</oboInOwl:hasOBONamespace>
        <oboInOwl:id>GAZ:00255909</oboInOwl:id>
        <rdfs:label>Mbareho</rdfs:label>
    </owl:NamedIndividual>
    


    <!-- http://purl.obolibrary.org/obo/GAZ_00255910 -->

    <owl:NamedIndividual rdf:about="http://purl.obolibrary.org/obo/GAZ_00255910">
        <obo:RO_0001025 rdf:resource="http://purl.obolibrary.org/obo/GAZ_00016898"/>
        <oboInOwl:hasOBONamespace>GAZ</oboInOwl:hasOBONamespace>
        <oboInOwl:id>GAZ:00255910</oboInOwl:id>
        <rdfs:label>Mbuini Tusu</rdfs:label>
    </owl:NamedIndividual>
    


    <!-- http://purl.obolibrary.org/obo/GAZ_00255911 -->

    <owl:NamedIndividual rdf:about="http://purl.obolibrary.org/obo/GAZ_00255911">
        <obo:RO_0001025 rdf:resource="http://purl.obolibrary.org/obo/GAZ_00016898"/>
        <obo:IAO_0000115>A harbor situated along the northwestern shore of the island of New Georgia in the Solomon Islands.</obo:IAO_0000115>
        <oboInOwl:hasOBONamespace>GAZ</oboInOwl:hasOBONamespace>
        <oboInOwl:id>GAZ:00255911</oboInOwl:id>
        <rdfs:label>Bairoko Harbor</rdfs:label>
    </owl:NamedIndividual>
    


    <!-- http://purl.obolibrary.org/obo/GAZ_00255912 -->

    <owl:NamedIndividual rdf:about="http://purl.obolibrary.org/obo/GAZ_00255912">
        <obo:RO_0001025 rdf:resource="http://purl.obolibrary.org/obo/GAZ_00005276"/>
        <obo:IAO_0000115>A river located in the northwest part of the island of Guadalcanal.</obo:IAO_0000115>
        <oboInOwl:hasOBONamespace>GAZ</oboInOwl:hasOBONamespace>
        <oboInOwl:id>GAZ:00255912</oboInOwl:id>
        <rdfs:label>Matanikau River</rdfs:label>
    </owl:NamedIndividual>
    


    <!-- http://purl.obolibrary.org/obo/GAZ_00255913 -->

    <owl:NamedIndividual rdf:about="http://purl.obolibrary.org/obo/GAZ_00255913">
        <obo:RO_0001025 rdf:resource="http://purl.obolibrary.org/obo/GAZ_00016898"/>
        <obo:IAO_0000115>The SW tip of the W end of New Georgia Island.</obo:IAO_0000115>
        <oboInOwl:hasOBONamespace>GAZ</oboInOwl:hasOBONamespace>
        <oboInOwl:id>GAZ:00255913</oboInOwl:id>
        <rdfs:label>Munda Point)</rdfs:label>
    </owl:NamedIndividual>
    


    <!-- http://purl.obolibrary.org/obo/GAZ_00255914 -->

    <owl:NamedIndividual rdf:about="http://purl.obolibrary.org/obo/GAZ_00255914">
        <rdf:type rdf:resource="http://purl.obolibrary.org/obo/ENVO_00000856"/>
        <obo:RO_0001025 rdf:resource="http://purl.obolibrary.org/obo/GAZ_00007206"/>
        <obo:IAO_0000115>A populated place. A village in the Solomon Islands, on Rennell Island.</obo:IAO_0000115>
        <oboInOwl:hasOBONamespace>GAZ</oboInOwl:hasOBONamespace>
        <oboInOwl:id>GAZ:00255914</oboInOwl:id>
        <rdfs:label>Abatai</rdfs:label>
    </owl:NamedIndividual>
    


    <!-- http://purl.obolibrary.org/obo/GAZ_00255915 -->

    <owl:NamedIndividual rdf:about="http://purl.obolibrary.org/obo/GAZ_00255915">
        <rdf:type rdf:resource="http://purl.obolibrary.org/obo/ENVO_00000856"/>
        <obo:RO_0001025 rdf:resource="http://purl.obolibrary.org/obo/GAZ_00007206"/>
        <obo:IAO_0000115>A populated place. A village.</obo:IAO_0000115>
        <oboInOwl:hasOBONamespace>GAZ</oboInOwl:hasOBONamespace>
        <oboInOwl:id>GAZ:00255915</oboInOwl:id>
        <rdfs:label>Tesauma</rdfs:label>
    </owl:NamedIndividual>
    


    <!-- http://purl.obolibrary.org/obo/GAZ_00255916 -->

    <owl:NamedIndividual rdf:about="http://purl.obolibrary.org/obo/GAZ_00255916">
        <rdf:type rdf:resource="http://purl.obolibrary.org/obo/ENVO_00000856"/>
        <obo:RO_0001025 rdf:resource="http://purl.obolibrary.org/obo/GAZ_00007206"/>
        <obo:IAO_0000115>A populated place. A village.</obo:IAO_0000115>
        <oboInOwl:hasOBONamespace>GAZ</oboInOwl:hasOBONamespace>
        <oboInOwl:id>GAZ:00255916</oboInOwl:id>
        <rdfs:label>Magino</rdfs:label>
    </owl:NamedIndividual>
    


    <!-- http://purl.obolibrary.org/obo/GAZ_00255917 -->

    <owl:NamedIndividual rdf:about="http://purl.obolibrary.org/obo/GAZ_00255917">
        <rdf:type rdf:resource="http://purl.obolibrary.org/obo/ENVO_00000856"/>
        <obo:RO_0001025 rdf:resource="http://purl.obolibrary.org/obo/GAZ_00007206"/>
        <obo:IAO_0000115>A populated place. A village.</obo:IAO_0000115>
        <oboInOwl:hasOBONamespace>GAZ</oboInOwl:hasOBONamespace>
        <oboInOwl:id>GAZ:00255917</oboInOwl:id>
        <rdfs:label>Matamoana</rdfs:label>
    </owl:NamedIndividual>
    


    <!-- http://purl.obolibrary.org/obo/GAZ_00255918 -->

    <owl:NamedIndividual rdf:about="http://purl.obolibrary.org/obo/GAZ_00255918">
        <rdf:type rdf:resource="http://purl.obolibrary.org/obo/ENVO_00000856"/>
        <obo:RO_0001025 rdf:resource="http://purl.obolibrary.org/obo/GAZ_00007206"/>
        <obo:IAO_0000115>A populated place. A village.</obo:IAO_0000115>
        <oboInOwl:hasOBONamespace>GAZ</oboInOwl:hasOBONamespace>
        <oboInOwl:id>GAZ:00255918</oboInOwl:id>
        <rdfs:label>Nukumatangi</rdfs:label>
    </owl:NamedIndividual>
    


    <!-- http://purl.obolibrary.org/obo/GAZ_00255919 -->

    <owl:NamedIndividual rdf:about="http://purl.obolibrary.org/obo/GAZ_00255919">
        <rdf:type rdf:resource="http://purl.obolibrary.org/obo/ENVO_00000856"/>
        <obo:RO_0001025 rdf:resource="http://purl.obolibrary.org/obo/GAZ_00007206"/>
        <obo:IAO_0000115>A populated place. A village.</obo:IAO_0000115>
        <oboInOwl:hasOBONamespace>GAZ</oboInOwl:hasOBONamespace>
        <oboInOwl:id>GAZ:00255919</oboInOwl:id>
        <rdfs:label>Gongona</rdfs:label>
    </owl:NamedIndividual>
    


    <!-- http://purl.obolibrary.org/obo/GAZ_00255920 -->

    <owl:NamedIndividual rdf:about="http://purl.obolibrary.org/obo/GAZ_00255920">
        <rdf:type rdf:resource="http://purl.obolibrary.org/obo/ENVO_00000856"/>
        <obo:RO_0001025 rdf:resource="http://purl.obolibrary.org/obo/GAZ_00005276"/>
        <obo:IAO_0000115>A populated place. A village on the island of Guadalcanal in the Solomon Islands.</obo:IAO_0000115>
        <oboInOwl:hasOBONamespace>GAZ</oboInOwl:hasOBONamespace>
        <oboInOwl:id>GAZ:00255920</oboInOwl:id>
        <rdfs:label>Kokumbona</rdfs:label>
    </owl:NamedIndividual>
    


    <!-- http://purl.obolibrary.org/obo/GAZ_00255921 -->

    <owl:NamedIndividual rdf:about="http://purl.obolibrary.org/obo/GAZ_00255921">
        <rdf:type rdf:resource="http://purl.obolibrary.org/obo/ENVO_00000856"/>
        <obo:RO_0001025 rdf:resource="http://purl.obolibrary.org/obo/GAZ_00007206"/>
        <obo:IAO_0000115>A populated place. A village.</obo:IAO_0000115>
        <oboInOwl:hasOBONamespace>GAZ</oboInOwl:hasOBONamespace>
        <oboInOwl:id>GAZ:00255921</oboInOwl:id>
        <rdfs:label>Moreno</rdfs:label>
    </owl:NamedIndividual>
    


    <!-- http://purl.obolibrary.org/obo/GAZ_00255922 -->

    <owl:NamedIndividual rdf:about="http://purl.obolibrary.org/obo/GAZ_00255922">
        <rdf:type rdf:resource="http://purl.obolibrary.org/obo/ENVO_00000856"/>
        <obo:RO_0001025 rdf:resource="http://purl.obolibrary.org/obo/GAZ_00007206"/>
        <obo:IAO_0000115>A populated place. A village in the Solomon Islands, on Rennell Island in the Rennell and Bellona province.</obo:IAO_0000115>
        <oboInOwl:hasOBONamespace>GAZ</oboInOwl:hasOBONamespace>
        <oboInOwl:id>GAZ:00255922</oboInOwl:id>
        <rdfs:label>Niupani</rdfs:label>
    </owl:NamedIndividual>
    


    <!-- http://purl.obolibrary.org/obo/GAZ_00255923 -->

    <owl:NamedIndividual rdf:about="http://purl.obolibrary.org/obo/GAZ_00255923">
        <rdf:type rdf:resource="http://purl.obolibrary.org/obo/ENVO_00000856"/>
        <obo:RO_0001025 rdf:resource="http://purl.obolibrary.org/obo/GAZ_00007206"/>
        <obo:IAO_0000115>A populated place. A village in the Solomon Islands, on Rennell Island in the Rennell and Bellona province.</obo:IAO_0000115>
        <oboInOwl:hasOBONamespace>GAZ</oboInOwl:hasOBONamespace>
        <oboInOwl:id>GAZ:00255923</oboInOwl:id>
        <rdfs:label>Teabamagu</rdfs:label>
    </owl:NamedIndividual>
    


    <!-- http://purl.obolibrary.org/obo/GAZ_00255924 -->

    <owl:NamedIndividual rdf:about="http://purl.obolibrary.org/obo/GAZ_00255924">
        <rdf:type rdf:resource="http://purl.obolibrary.org/obo/ENVO_00000856"/>
        <obo:RO_0001025 rdf:resource="http://purl.obolibrary.org/obo/GAZ_00007206"/>
        <obo:IAO_0000115>A populated place. A village in the Solomon Islands, on Rennell Island in the Rennell and Bellona province.</obo:IAO_0000115>
        <oboInOwl:hasOBONamespace>GAZ</oboInOwl:hasOBONamespace>
        <oboInOwl:id>GAZ:00255924</oboInOwl:id>
        <rdfs:label>Tebaitahe</rdfs:label>
    </owl:NamedIndividual>
    


    <!-- http://purl.obolibrary.org/obo/GAZ_00255926 -->

    <owl:NamedIndividual rdf:about="http://purl.obolibrary.org/obo/GAZ_00255926">
        <obo:RO_0001025 rdf:resource="http://purl.obolibrary.org/obo/GAZ_00005276"/>
        <obo:IAO_0000115>The Capital Territory of the Solomon Islands.</obo:IAO_0000115>
        <oboInOwl:hasOBONamespace>GAZ</oboInOwl:hasOBONamespace>
        <oboInOwl:id>GAZ:00255926</oboInOwl:id>
        <rdfs:label>Capital Territory</rdfs:label>
    </owl:NamedIndividual>
    


    <!-- http://purl.obolibrary.org/obo/GAZ_00255927 -->

    <owl:NamedIndividual rdf:about="http://purl.obolibrary.org/obo/GAZ_00255927">
        <obo:RO_0001025 rdf:resource="http://purl.obolibrary.org/obo/GAZ_00016907"/>
        <obo:IAO_0000115>A protected area.</obo:IAO_0000115>
        <oboInOwl:hasOBONamespace>GAZ</oboInOwl:hasOBONamespace>
        <oboInOwl:id>GAZ:00255927</oboInOwl:id>
        <rdfs:label>Kolombangara Forest Reserve</rdfs:label>
    </owl:NamedIndividual>
    


    <!-- http://purl.obolibrary.org/obo/GAZ_00255928 -->

    <owl:NamedIndividual rdf:about="http://purl.obolibrary.org/obo/GAZ_00255928">
        <rdf:type rdf:resource="http://purl.obolibrary.org/obo/ENVO_00000220"/>
        <obo:RO_0001025 rdf:resource="http://purl.obolibrary.org/obo/GAZ_00255762"/>
        <obo:IAO_0000115>An island group.</obo:IAO_0000115>
        <oboInOwl:hasOBONamespace>GAZ</oboInOwl:hasOBONamespace>
        <oboInOwl:id>GAZ:00255928</oboInOwl:id>
        <rdfs:label>Arnavon Islands</rdfs:label>
    </owl:NamedIndividual>
    


    <!-- http://purl.obolibrary.org/obo/GAZ_00255929 -->

    <owl:NamedIndividual rdf:about="http://purl.obolibrary.org/obo/GAZ_00255929">
        <obo:RO_0001025 rdf:resource="http://purl.obolibrary.org/obo/GAZ_00255928"/>
        <obo:IAO_0000115>A protected area. Located in Manning Strait between Isabel &amp; Choiseul Islands. Encompasses the three Arnavon Islands, Kerehikapa, Sikopo, and Maleivona. Established 1985.</obo:IAO_0000115>
        <oboInOwl:hasOBONamespace>GAZ</oboInOwl:hasOBONamespace>
        <oboInOwl:id>GAZ:00255929</oboInOwl:id>
        <rdfs:label>Arnavon Islands Marine Conservation Area</rdfs:label>
    </owl:NamedIndividual>
    


    <!-- http://purl.obolibrary.org/obo/GAZ_00255930 -->

    <owl:NamedIndividual rdf:about="http://purl.obolibrary.org/obo/GAZ_00255930">
        <obo:RO_0001025 rdf:resource="http://purl.obolibrary.org/obo/GAZ_00016910"/>
        <obo:IAO_0000115>An island.</obo:IAO_0000115>
        <oboInOwl:hasOBONamespace>GAZ</oboInOwl:hasOBONamespace>
        <oboInOwl:id>GAZ:00255930</oboInOwl:id>
        <rdfs:label>Njanjelakalau Island</rdfs:label>
    </owl:NamedIndividual>
    


    <!-- http://purl.obolibrary.org/obo/GAZ_00255932 -->

    <owl:NamedIndividual rdf:about="http://purl.obolibrary.org/obo/GAZ_00255932">
        <obo:RO_0001025 rdf:resource="http://purl.obolibrary.org/obo/GAZ_00016910"/>
        <obo:IAO_0000115>An island.</obo:IAO_0000115>
        <oboInOwl:hasOBONamespace>GAZ</oboInOwl:hasOBONamespace>
        <oboInOwl:id>GAZ:00255932</oboInOwl:id>
        <rdfs:label>Njanjelakalonga Island</rdfs:label>
    </owl:NamedIndividual>
    


    <!-- http://purl.obolibrary.org/obo/GAZ_00255933 -->

    <owl:NamedIndividual rdf:about="http://purl.obolibrary.org/obo/GAZ_00255933">
        <obo:RO_0001025 rdf:resource="http://purl.obolibrary.org/obo/GAZ_00005276"/>
        <obo:IAO_0000115>A protected area. Located approximately 20 km from Honiara . Established 1994.</obo:IAO_0000115>
        <oboInOwl:hasOBONamespace>GAZ</oboInOwl:hasOBONamespace>
        <oboInOwl:id>GAZ:00255933</oboInOwl:id>
        <rdfs:label>Komarindi Conservation Area</rdfs:label>
    </owl:NamedIndividual>
    


    <!-- http://purl.obolibrary.org/obo/GAZ_00255934 -->

    <owl:NamedIndividual rdf:about="http://purl.obolibrary.org/obo/GAZ_00255934">
        <obo:RO_0001025 rdf:resource="http://purl.obolibrary.org/obo/GAZ_00016911"/>
        <obo:IAO_0000115>A protected area.</obo:IAO_0000115>
        <oboInOwl:hasOBONamespace>GAZ</oboInOwl:hasOBONamespace>
        <oboInOwl:id>GAZ:00255934</oboInOwl:id>
        <rdfs:label>Tulagi Bird Sanctuary</rdfs:label>
    </owl:NamedIndividual>
    


    <!-- http://purl.obolibrary.org/obo/GAZ_00255935 -->

    <owl:NamedIndividual rdf:about="http://purl.obolibrary.org/obo/GAZ_00255935">
        <obo:RO_0001025 rdf:resource="http://purl.obolibrary.org/obo/GAZ_00009134"/>
        <obo:IAO_0000115>A protected area.</obo:IAO_0000115>
        <oboInOwl:hasOBONamespace>GAZ</oboInOwl:hasOBONamespace>
        <oboInOwl:id>GAZ:00255935</oboInOwl:id>
        <rdfs:label>Makira Community Forest Management Area</rdfs:label>
    </owl:NamedIndividual>
    


    <!-- http://purl.obolibrary.org/obo/GAZ_00255936 -->

    <owl:NamedIndividual rdf:about="http://purl.obolibrary.org/obo/GAZ_00255936">
        <obo:RO_0001025 rdf:resource="http://purl.obolibrary.org/obo/GAZ_00016910"/>
        <obo:IAO_0000115>An island.</obo:IAO_0000115>
        <oboInOwl:hasOBONamespace>GAZ</oboInOwl:hasOBONamespace>
        <oboInOwl:id>GAZ:00255936</oboInOwl:id>
        <rdfs:label>Mandoleana Island</rdfs:label>
    </owl:NamedIndividual>
    


    <!-- http://purl.obolibrary.org/obo/GAZ_00255937 -->

    <owl:NamedIndividual rdf:about="http://purl.obolibrary.org/obo/GAZ_00255937">
        <obo:RO_0001025 rdf:resource="http://purl.obolibrary.org/obo/GAZ_00255936"/>
        <obo:IAO_0000115>A protected area.</obo:IAO_0000115>
        <oboInOwl:hasOBONamespace>GAZ</oboInOwl:hasOBONamespace>
        <oboInOwl:id>GAZ:00255937</oboInOwl:id>
        <rdfs:label>Mandoliana Bird Sanctuary</rdfs:label>
    </owl:NamedIndividual>
    


    <!-- http://purl.obolibrary.org/obo/GAZ_00255938 -->

    <owl:NamedIndividual rdf:about="http://purl.obolibrary.org/obo/GAZ_00255938">
        <obo:RO_0001025 rdf:resource="http://purl.obolibrary.org/obo/GAZ_00009132"/>
        <obo:IAO_0000115>An atoll.</obo:IAO_0000115>
        <oboInOwl:hasOBONamespace>GAZ</oboInOwl:hasOBONamespace>
        <oboInOwl:id>GAZ:00255938</oboInOwl:id>
        <rdfs:label>Oema Atoll</rdfs:label>
    </owl:NamedIndividual>
    


    <!-- http://purl.obolibrary.org/obo/GAZ_00255939 -->

    <owl:NamedIndividual rdf:about="http://purl.obolibrary.org/obo/GAZ_00255939">
        <obo:RO_0001025 rdf:resource="http://purl.obolibrary.org/obo/GAZ_00007206"/>
        <obo:IAO_0000115>A protected area. It covers the eastern third of Rennell Island with boundaries extending seawards for 3 nautical miles. Established 1998.</obo:IAO_0000115>
        <oboInOwl:hasOBONamespace>GAZ</oboInOwl:hasOBONamespace>
        <oboInOwl:id>GAZ:00255939</oboInOwl:id>
        <rdfs:label>East Rennell World Heritage Area</rdfs:label>
    </owl:NamedIndividual>
    


    <!-- http://purl.obolibrary.org/obo/GAZ_00255940 -->

    <owl:NamedIndividual rdf:about="http://purl.obolibrary.org/obo/GAZ_00255940">
        <obo:RO_0001025 rdf:resource="http://purl.obolibrary.org/obo/GAZ_00005276"/>
        <obo:IAO_0000115>A protected area. Established 1964.</obo:IAO_0000115>
        <oboInOwl:hasOBONamespace>GAZ</oboInOwl:hasOBONamespace>
        <oboInOwl:id>GAZ:00255940</oboInOwl:id>
        <rdfs:label>Queen Elizabeth National Park</rdfs:label>
    </owl:NamedIndividual>
    


    <!-- http://purl.obolibrary.org/obo/GAZ_00255941 -->

    <owl:NamedIndividual rdf:about="http://purl.obolibrary.org/obo/GAZ_00255941">
        <obo:RO_0001025 rdf:resource="http://purl.obolibrary.org/obo/GAZ_00012782"/>
        <obo:IAO_0000115>An island N of Santa Isabel Island.</obo:IAO_0000115>
        <oboInOwl:hasOBONamespace>GAZ</oboInOwl:hasOBONamespace>
        <oboInOwl:id>GAZ:00255941</oboInOwl:id>
        <rdfs:label>Barora Ite Island</rdfs:label>
    </owl:NamedIndividual>
    


    <!-- http://purl.obolibrary.org/obo/GAZ_00255942 -->

    <owl:NamedIndividual rdf:about="http://purl.obolibrary.org/obo/GAZ_00255942">
        <obo:RO_0001025 rdf:resource="http://purl.obolibrary.org/obo/GAZ_00012782"/>
        <obo:IAO_0000115>An island N of Santa Isabel Island.</obo:IAO_0000115>
        <oboInOwl:hasOBONamespace>GAZ</oboInOwl:hasOBONamespace>
        <oboInOwl:id>GAZ:00255942</oboInOwl:id>
        <rdfs:label>Barora Fa</rdfs:label>
    </owl:NamedIndividual>
    


    <!-- http://purl.obolibrary.org/obo/GAZ_00255943 -->

    <owl:NamedIndividual rdf:about="http://purl.obolibrary.org/obo/GAZ_00255943">
        <obo:RO_0001025 rdf:resource="http://purl.obolibrary.org/obo/GAZ_00012782"/>
        <obo:IAO_0000115>An island N of Santa Isabel island.</obo:IAO_0000115>
        <oboInOwl:hasOBONamespace>GAZ</oboInOwl:hasOBONamespace>
        <oboInOwl:id>GAZ:00255943</oboInOwl:id>
        <rdfs:label>Ghaghe Island</rdfs:label>
    </owl:NamedIndividual>
    


    <!-- http://purl.obolibrary.org/obo/GAZ_00255944 -->

    <owl:NamedIndividual rdf:about="http://purl.obolibrary.org/obo/GAZ_00255944">
        <obo:RO_0001025 rdf:resource="http://purl.obolibrary.org/obo/GAZ_00012782"/>
        <obo:IAO_0000115>A channel between the islands of Isabel and San Jorge, Isabel Province.</obo:IAO_0000115>
        <oboInOwl:hasOBONamespace>GAZ</oboInOwl:hasOBONamespace>
        <oboInOwl:id>GAZ:00255944</oboInOwl:id>
        <rdfs:label>Ortega Channel</rdfs:label>
    </owl:NamedIndividual>
    


    <!-- http://purl.obolibrary.org/obo/GAZ_00255945 -->

    <owl:NamedIndividual rdf:about="http://purl.obolibrary.org/obo/GAZ_00255945">
        <obo:RO_0001025 rdf:resource="http://purl.obolibrary.org/obo/GAZ_00005276"/>
        <obo:IAO_0000115>A freshwater lagoon. Located on the southeast coast of Guadalcanal, Guadalcanal Province.</obo:IAO_0000115>
        <oboInOwl:hasOBONamespace>GAZ</oboInOwl:hasOBONamespace>
        <oboInOwl:id>GAZ:00255945</oboInOwl:id>
        <rdfs:label>Lauvi Lagoon</rdfs:label>
    </owl:NamedIndividual>
    


    <!-- http://purl.obolibrary.org/obo/GAZ_00255946 -->

    <owl:NamedIndividual rdf:about="http://purl.obolibrary.org/obo/GAZ_00255946">
        <obo:RO_0001025 rdf:resource="http://purl.obolibrary.org/obo/GAZ_00009137"/>
        <obo:IAO_0000115>A long narrow coastal lagoon with many barrier islands and fringing mangroves. Located along the southwestern coast of Malaita.</obo:IAO_0000115>
        <oboInOwl:hasOBONamespace>GAZ</oboInOwl:hasOBONamespace>
        <oboInOwl:id>GAZ:00255946</oboInOwl:id>
        <rdfs:label>Are&apos;Are Lagoon</rdfs:label>
    </owl:NamedIndividual>
    


    <!-- http://purl.obolibrary.org/obo/GAZ_00255947 -->

    <owl:NamedIndividual rdf:about="http://purl.obolibrary.org/obo/GAZ_00255947">
        <obo:RO_0001025 rdf:resource="http://purl.obolibrary.org/obo/GAZ_00009137"/>
        <obo:IAO_0000115>A lagoon. Located at the N end of the Maramasike Passage.</obo:IAO_0000115>
        <oboInOwl:hasOBONamespace>GAZ</oboInOwl:hasOBONamespace>
        <oboInOwl:id>GAZ:00255947</oboInOwl:id>
        <rdfs:label>Raroi Su&apos;u Lagoon</rdfs:label>
    </owl:NamedIndividual>
    


    <!-- http://purl.obolibrary.org/obo/GAZ_00255948 -->

    <owl:NamedIndividual rdf:about="http://purl.obolibrary.org/obo/GAZ_00255948">
        <obo:RO_0001025 rdf:resource="http://purl.obolibrary.org/obo/GAZ_00009134"/>
        <obo:IAO_0000115>A wetland. A number of extensive freshwater swamps in broad river valleys in the lowlands and foothills of western Makira. Located in the interior of west-central Makira, Makira Province.</obo:IAO_0000115>
        <oboInOwl:hasOBONamespace>GAZ</oboInOwl:hasOBONamespace>
        <oboInOwl:id>GAZ:00255948</oboInOwl:id>
        <rdfs:label>Makira Swamps</rdfs:label>
    </owl:NamedIndividual>
    


    <!-- http://purl.obolibrary.org/obo/GAZ_00255949 -->

    <owl:NamedIndividual rdf:about="http://purl.obolibrary.org/obo/GAZ_00255949">
        <obo:RO_0001025 rdf:resource="http://purl.obolibrary.org/obo/GAZ_00016905"/>
        <oboInOwl:hasOBONamespace>GAZ</oboInOwl:hasOBONamespace>
        <oboInOwl:id>GAZ:00255949</oboInOwl:id>
        <rdfs:label>Mount Matindingi</rdfs:label>
    </owl:NamedIndividual>
    


    <!-- http://purl.obolibrary.org/obo/GAZ_00255950 -->

    <owl:NamedIndividual rdf:about="http://purl.obolibrary.org/obo/GAZ_00255950">
        <obo:RO_0001025 rdf:resource="http://purl.obolibrary.org/obo/GAZ_00016895"/>
        <obo:IAO_0000115>A lake.</obo:IAO_0000115>
        <oboInOwl:hasOBONamespace>GAZ</oboInOwl:hasOBONamespace>
        <oboInOwl:id>GAZ:00255950</oboInOwl:id>
        <rdfs:label>Lake Rano</rdfs:label>
    </owl:NamedIndividual>
    


    <!-- http://purl.obolibrary.org/obo/GAZ_00255951 -->

    <owl:NamedIndividual rdf:about="http://purl.obolibrary.org/obo/GAZ_00255951">
        <obo:RO_0001025 rdf:resource="http://purl.obolibrary.org/obo/GAZ_00005276"/>
        <obo:IAO_0000115>A freshwater lake. Located in the east-central highlands of Guadalcanal, Guadalcanal Province.</obo:IAO_0000115>
        <oboInOwl:hasOBONamespace>GAZ</oboInOwl:hasOBONamespace>
        <oboInOwl:id>GAZ:00255951</oboInOwl:id>
        <rdfs:label>Lee&apos;s Lake</rdfs:label>
    </owl:NamedIndividual>
    


    <!-- http://purl.obolibrary.org/obo/GAZ_00255952 -->

    <owl:NamedIndividual rdf:about="http://purl.obolibrary.org/obo/GAZ_00255952">
        <obo:RO_0001025 rdf:resource="http://purl.obolibrary.org/obo/GAZ_00255780"/>
        <obo:IAO_0000115>One of the Three Sisters Islands.</obo:IAO_0000115>
        <oboInOwl:hasOBONamespace>GAZ</oboInOwl:hasOBONamespace>
        <oboInOwl:id>GAZ:00255952</oboInOwl:id>
        <rdfs:label>Malaupaina Island</rdfs:label>
    </owl:NamedIndividual>
    


    <!-- http://purl.obolibrary.org/obo/GAZ_00255953 -->

    <owl:NamedIndividual rdf:about="http://purl.obolibrary.org/obo/GAZ_00255953">
        <obo:RO_0001025 rdf:resource="http://purl.obolibrary.org/obo/GAZ_00255780"/>
        <obo:IAO_0000115>One of the Three Sisters Islands.</obo:IAO_0000115>
        <oboInOwl:hasOBONamespace>GAZ</oboInOwl:hasOBONamespace>
        <oboInOwl:id>GAZ:00255953</oboInOwl:id>
        <rdfs:label>Malaulalo Island</rdfs:label>
    </owl:NamedIndividual>
    


    <!-- http://purl.obolibrary.org/obo/GAZ_00255954 -->

    <owl:NamedIndividual rdf:about="http://purl.obolibrary.org/obo/GAZ_00255954">
        <obo:RO_0001025 rdf:resource="http://purl.obolibrary.org/obo/GAZ_00255780"/>
        <obo:IAO_0000115>One of the Three Sisters Islands.</obo:IAO_0000115>
        <oboInOwl:hasOBONamespace>GAZ</oboInOwl:hasOBONamespace>
        <oboInOwl:id>GAZ:00255954</oboInOwl:id>
        <rdfs:label>Ali&apos;ite Island</rdfs:label>
    </owl:NamedIndividual>
    


    <!-- http://purl.obolibrary.org/obo/GAZ_00255955 -->

    <owl:NamedIndividual rdf:about="http://purl.obolibrary.org/obo/GAZ_00255955">
        <obo:RO_0001025 rdf:resource="http://purl.obolibrary.org/obo/GAZ_00009134"/>
        <obo:IAO_0000115>A bay in the SW of Makira Island.</obo:IAO_0000115>
        <oboInOwl:hasOBONamespace>GAZ</oboInOwl:hasOBONamespace>
        <oboInOwl:id>GAZ:00255955</oboInOwl:id>
        <rdfs:label>Star Harbour</rdfs:label>
    </owl:NamedIndividual>
    


    <!-- http://purl.obolibrary.org/obo/GAZ_00255956 -->

    <owl:NamedIndividual rdf:about="http://purl.obolibrary.org/obo/GAZ_00255956">
        <obo:RO_0001025 rdf:resource="http://purl.obolibrary.org/obo/GAZ_00009143"/>
        <obo:IAO_0000115>A lake.</obo:IAO_0000115>
        <oboInOwl:hasOBONamespace>GAZ</oboInOwl:hasOBONamespace>
        <oboInOwl:id>GAZ:00255956</oboInOwl:id>
        <rdfs:label>Lake Wairata</rdfs:label>
    </owl:NamedIndividual>
    


    <!-- 
    ///////////////////////////////////////////////////////////////////////////////////////
    //
    // Annotations
    //
    ///////////////////////////////////////////////////////////////////////////////////////
     -->

    <rdf:Description rdf:about="http://purl.obolibrary.org/obo/GAZ_00009554">
        <oboInOwl:id>GAZ:00009554</oboInOwl:id>
        <rdfs:label>Province (Solomon Islands)</rdfs:label>
        <oboInOwl:hasOBONamespace>GAZ</oboInOwl:hasOBONamespace>
    </rdf:Description>
    <rdf:Description rdf:about="http://purl.obolibrary.org/obo/GAZ_00009555">
        <oboInOwl:id>GAZ:00009555</oboInOwl:id>
        <obo:IAO_0000115>One of the provinces of the Solomon Islands, consisting of the island of Guadalcanal.</obo:IAO_0000115>
        <rdfs:label>Guadalcanal Province</rdfs:label>
        <oboInOwl:hasOBONamespace>GAZ</oboInOwl:hasOBONamespace>
    </rdf:Description>
    <rdf:Description rdf:about="http://purl.obolibrary.org/obo/GAZ_00009556">
        <obo:IAO_0000115>A Province of the Solomon Islands.</obo:IAO_0000115>
        <oboInOwl:id>GAZ:00009556</oboInOwl:id>
        <rdfs:label>Rennell and Bellona Province</rdfs:label>
        <oboInOwl:hasOBONamespace>GAZ</oboInOwl:hasOBONamespace>
    </rdf:Description>
    <rdf:Description rdf:about="http://purl.obolibrary.org/obo/GAZ_00009557">
        <oboInOwl:id>GAZ:00009557</oboInOwl:id>
        <rdfs:label>Temotu Province</rdfs:label>
        <oboInOwl:hasOBONamespace>GAZ</oboInOwl:hasOBONamespace>
        <obo:IAO_0000115>The easternmost province of the Solomon Islands.</obo:IAO_0000115>
    </rdf:Description>
    <rdf:Description rdf:about="http://purl.obolibrary.org/obo/GAZ_00009558">
        <oboInOwl:id>GAZ:00009558</oboInOwl:id>
        <obo:IAO_0000115>One of the provinces of the Solomon Islands.</obo:IAO_0000115>
        <oboInOwl:hasOBONamespace>GAZ</oboInOwl:hasOBONamespace>
        <rdfs:label>Malaita Province</rdfs:label>
    </rdf:Description>
    <rdf:Description rdf:about="http://purl.obolibrary.org/obo/GAZ_00012779">
        <obo:IAO_0000115>One of the provinces of the Solomon Islands. The main part of the province is Makira Island.</obo:IAO_0000115>
        <rdfs:label>Makira-Ulawa Province</rdfs:label>
        <oboInOwl:id>GAZ:00012779</oboInOwl:id>
        <oboInOwl:hasOBONamespace>GAZ</oboInOwl:hasOBONamespace>
    </rdf:Description>
    <rdf:Description rdf:about="http://purl.obolibrary.org/obo/GAZ_00012780">
        <obo:IAO_0000115>One of the nine provinces of the Solomon Islands. It lies between the island of Bougainville (part of Papua New Guinea) and Santa Isabel in the west of the Solomon Islands.</obo:IAO_0000115>
        <oboInOwl:hasOBONamespace>GAZ</oboInOwl:hasOBONamespace>
        <rdfs:label>Choiseul Province</rdfs:label>
        <oboInOwl:id>GAZ:00012780</oboInOwl:id>
    </rdf:Description>
    <rdf:Description rdf:about="http://purl.obolibrary.org/obo/GAZ_00012781">
        <oboInOwl:hasOBONamespace>GAZ</oboInOwl:hasOBONamespace>
        <rdfs:label>Western Province</rdfs:label>
        <oboInOwl:id>GAZ:00012781</oboInOwl:id>
        <obo:IAO_0000115>The largest of the provinces of the Solomon Islands.</obo:IAO_0000115>
    </rdf:Description>
    <rdf:Description rdf:about="http://purl.obolibrary.org/obo/GAZ_00012782">
        <oboInOwl:hasOBONamespace>GAZ</oboInOwl:hasOBONamespace>
        <rdfs:label>Isabel Province</rdfs:label>
        <obo:IAO_0000115>One of the provinces of the Solomon Islands.</obo:IAO_0000115>
        <oboInOwl:id>GAZ:00012782</oboInOwl:id>
    </rdf:Description>
    <rdf:Description rdf:about="http://purl.obolibrary.org/obo/GAZ_00012783">
        <oboInOwl:id>GAZ:00012783</oboInOwl:id>
        <rdfs:label>Central Province</rdfs:label>
        <obo:IAO_0000115>One of the provinces of the Solomon Islands, covering the Russell Islands, Nggella (Florida Islands) and Savo Island.</obo:IAO_0000115>
        <oboInOwl:hasOBONamespace>GAZ</oboInOwl:hasOBONamespace>
    </rdf:Description>
</rdf:RDF>



<!-- Generated by the OWL API (version 4.5.6) https://github.com/owlcs/owlapi -->

