<?xml version="1.0"?>
<rdf:RDF xmlns="http://purl.obolibrary.org/obo/gaz/subsets/countries/Sudan.owl#"
     xml:base="http://purl.obolibrary.org/obo/gaz/subsets/countries/Sudan.owl"
     xmlns:obo="http://purl.obolibrary.org/obo/"
     xmlns:owl="http://www.w3.org/2002/07/owl#"
     xmlns:rdf="http://www.w3.org/1999/02/22-rdf-syntax-ns#"
     xmlns:xml="http://www.w3.org/XML/1998/namespace"
     xmlns:xsd="http://www.w3.org/2001/XMLSchema#"
     xmlns:rdfs="http://www.w3.org/2000/01/rdf-schema#"
     xmlns:oboInOwl="http://www.geneontology.org/formats/oboInOwl#">
    <owl:Ontology rdf:about="http://purl.obolibrary.org/obo/gaz/subsets/countries/Sudan.owl">
        <owl:imports rdf:resource="http://purl.obolibrary.org/obo/gaz/imports/envo_import.owl"/>
        <owl:imports rdf:resource="http://purl.obolibrary.org/obo/gaz/imports/ro_import.owl"/>
    </owl:Ontology>
    


    <!-- 
    ///////////////////////////////////////////////////////////////////////////////////////
    //
    // Annotation properties
    //
    ///////////////////////////////////////////////////////////////////////////////////////
     -->

    


    <!-- http://purl.obolibrary.org/obo/IAO_0000115 -->

    <owl:AnnotationProperty rdf:about="http://purl.obolibrary.org/obo/IAO_0000115"/>
    


    <!-- http://www.geneontology.org/formats/oboInOwl#hasOBONamespace -->

    <owl:AnnotationProperty rdf:about="http://www.geneontology.org/formats/oboInOwl#hasOBONamespace"/>
    


    <!-- http://www.geneontology.org/formats/oboInOwl#id -->

    <owl:AnnotationProperty rdf:about="http://www.geneontology.org/formats/oboInOwl#id"/>
    


    <!-- 
    ///////////////////////////////////////////////////////////////////////////////////////
    //
    // Object Properties
    //
    ///////////////////////////////////////////////////////////////////////////////////////
     -->

    


    <!-- http://purl.obolibrary.org/obo/RO_0001025 -->

    <owl:ObjectProperty rdf:about="http://purl.obolibrary.org/obo/RO_0001025"/>
    


    <!-- 
    ///////////////////////////////////////////////////////////////////////////////////////
    //
    // Classes
    //
    ///////////////////////////////////////////////////////////////////////////////////////
     -->

    


    <!-- http://purl.obolibrary.org/obo/ENVO_00000004 -->

    <owl:Class rdf:about="http://purl.obolibrary.org/obo/ENVO_00000004"/>
    


    <!-- http://purl.obolibrary.org/obo/ENVO_00000009 -->

    <owl:Class rdf:about="http://purl.obolibrary.org/obo/ENVO_00000009"/>
    


    <!-- http://purl.obolibrary.org/obo/ENVO_00000033 -->

    <owl:Class rdf:about="http://purl.obolibrary.org/obo/ENVO_00000033"/>
    


    <!-- http://purl.obolibrary.org/obo/ENVO_00000074 -->

    <owl:Class rdf:about="http://purl.obolibrary.org/obo/ENVO_00000074"/>
    


    <!-- http://purl.obolibrary.org/obo/ENVO_00000106 -->

    <owl:Class rdf:about="http://purl.obolibrary.org/obo/ENVO_00000106"/>
    


    <!-- http://purl.obolibrary.org/obo/ENVO_00000220 -->

    <owl:Class rdf:about="http://purl.obolibrary.org/obo/ENVO_00000220"/>
    


    <!-- http://purl.obolibrary.org/obo/ENVO_00000222 -->

    <owl:Class rdf:about="http://purl.obolibrary.org/obo/ENVO_00000222"/>
    


    <!-- http://purl.obolibrary.org/obo/ENVO_00000475 -->

    <owl:Class rdf:about="http://purl.obolibrary.org/obo/ENVO_00000475"/>
    


    <!-- http://purl.obolibrary.org/obo/ENVO_00000856 -->

    <owl:Class rdf:about="http://purl.obolibrary.org/obo/ENVO_00000856"/>
    


    <!-- http://purl.obolibrary.org/obo/GAZ_00007859 -->

    <owl:Class rdf:about="http://purl.obolibrary.org/obo/GAZ_00007859"/>
    


    <!-- http://purl.obolibrary.org/obo/GAZ_00007860 -->

    <owl:Class rdf:about="http://purl.obolibrary.org/obo/GAZ_00007860">
        <rdfs:subClassOf rdf:resource="http://purl.obolibrary.org/obo/GAZ_00007859"/>
    </owl:Class>
    


    <!-- http://purl.obolibrary.org/obo/GAZ_00058884 -->

    <owl:Class rdf:about="http://purl.obolibrary.org/obo/GAZ_00058884"/>
    


    <!-- http://purl.obolibrary.org/obo/GAZ_00058885 -->

    <owl:Class rdf:about="http://purl.obolibrary.org/obo/GAZ_00058885">
        <rdfs:subClassOf rdf:resource="http://purl.obolibrary.org/obo/GAZ_00058884"/>
        <obo:IAO_0000115>A cataract on the River Nile in Sudan near the confluence with the Atbara River.</obo:IAO_0000115>
        <oboInOwl:hasOBONamespace>GAZ</oboInOwl:hasOBONamespace>
        <oboInOwl:id>GAZ:00058885</oboInOwl:id>
        <rdfs:label>Fifth Cataract</rdfs:label>
    </owl:Class>
    


    <!-- http://purl.obolibrary.org/obo/GAZ_00058886 -->

    <owl:Class rdf:about="http://purl.obolibrary.org/obo/GAZ_00058886">
        <rdfs:subClassOf rdf:resource="http://purl.obolibrary.org/obo/GAZ_00058884"/>
    </owl:Class>
    


    <!-- http://purl.obolibrary.org/obo/GAZ_00058887 -->

    <owl:Class rdf:about="http://purl.obolibrary.org/obo/GAZ_00058887">
        <rdfs:subClassOf rdf:resource="http://purl.obolibrary.org/obo/GAZ_00058884"/>
        <obo:IAO_0000115>A former cataract on the River Nile in Sudan that was in Nubia and is now submerged in Lake Nasser.</obo:IAO_0000115>
        <oboInOwl:hasOBONamespace>GAZ</oboInOwl:hasOBONamespace>
        <oboInOwl:id>GAZ:00058887</oboInOwl:id>
        <rdfs:label>Second Cataract</rdfs:label>
    </owl:Class>
    


    <!-- http://purl.obolibrary.org/obo/GAZ_00058888 -->

    <owl:Class rdf:about="http://purl.obolibrary.org/obo/GAZ_00058888">
        <rdfs:subClassOf rdf:resource="http://purl.obolibrary.org/obo/GAZ_00058884"/>
        <obo:IAO_0000115>A cataract on the River Nile in Sudan near Tombos.</obo:IAO_0000115>
        <oboInOwl:hasOBONamespace>GAZ</oboInOwl:hasOBONamespace>
        <oboInOwl:id>GAZ:00058888</oboInOwl:id>
        <rdfs:label>Third Cataract</rdfs:label>
    </owl:Class>
    


    <!-- http://purl.obolibrary.org/obo/GAZ_00058889 -->

    <owl:Class rdf:about="http://purl.obolibrary.org/obo/GAZ_00058889">
        <rdfs:subClassOf rdf:resource="http://purl.obolibrary.org/obo/GAZ_00058884"/>
        <obo:IAO_0000115>A cataract on the River Nile in Sudan where it cuts through the Sabaluka pluton near Bagrawiyah.</obo:IAO_0000115>
        <oboInOwl:hasOBONamespace>GAZ</oboInOwl:hasOBONamespace>
        <oboInOwl:id>GAZ:00058889</oboInOwl:id>
        <rdfs:label>Sixth Cataract</rdfs:label>
    </owl:Class>
    


    <!-- http://purl.obolibrary.org/obo/GAZ_00058890 -->

    <owl:Class rdf:about="http://purl.obolibrary.org/obo/GAZ_00058890">
        <rdfs:subClassOf rdf:resource="http://purl.obolibrary.org/obo/GAZ_00058884"/>
    </owl:Class>
    


    <!-- http://purl.obolibrary.org/obo/GAZ_00230472 -->

    <owl:Class rdf:about="http://purl.obolibrary.org/obo/GAZ_00230472">
        <obo:IAO_0000115>A river. A tributary of the Qechene River.</obo:IAO_0000115>
        <oboInOwl:hasOBONamespace>GAZ</oboInOwl:hasOBONamespace>
        <oboInOwl:id>GAZ:00230472</oboInOwl:id>
        <rdfs:label>Ketama River</rdfs:label>
    </owl:Class>
    


    <!-- http://purl.obolibrary.org/obo/GAZ_00230473 -->

    <owl:Class rdf:about="http://purl.obolibrary.org/obo/GAZ_00230473">
        <obo:IAO_0000115>A river. A tributary of the Qechene River.</obo:IAO_0000115>
        <oboInOwl:hasOBONamespace>GAZ</oboInOwl:hasOBONamespace>
        <oboInOwl:id>GAZ:00230473</oboInOwl:id>
        <rdfs:label>Woia River</rdfs:label>
    </owl:Class>
    


    <!-- 
    ///////////////////////////////////////////////////////////////////////////////////////
    //
    // Individuals
    //
    ///////////////////////////////////////////////////////////////////////////////////////
     -->

    


    <!-- http://purl.obolibrary.org/obo/GAZ_00000560 -->

    <owl:NamedIndividual rdf:about="http://purl.obolibrary.org/obo/GAZ_00000560">
        <rdf:type rdf:resource="http://purl.obolibrary.org/obo/ENVO_00000009"/>
        <obo:IAO_0000115>A country in North Africa. It is bordered by Egypt to the north, the Red Sea to the northeast, Eritrea and Ethiopia to the east, Kenya and Uganda to the southeast, Democratic Republic of the Congo and the Central African Republic to the southwest, Chad to the west and Libya to the northwest. Sudan is divided into twenty-six states (wilayat, singular wilayah) which in turn are subdivided into 133 districts.</obo:IAO_0000115>
        <oboInOwl:hasOBONamespace>GAZ</oboInOwl:hasOBONamespace>
        <oboInOwl:id>GAZ:00000560</oboInOwl:id>
        <rdfs:label>Sudan</rdfs:label>
    </owl:NamedIndividual>
    


    <!-- http://purl.obolibrary.org/obo/GAZ_00000672 -->

    <owl:NamedIndividual rdf:about="http://purl.obolibrary.org/obo/GAZ_00000672">
        <obo:RO_0001025 rdf:resource="http://purl.obolibrary.org/obo/GAZ_00233441"/>
        <obo:IAO_0000115>One of the states of Sudan. It lies between the Blue Nile and the White Nile in the east-central region of the country.</obo:IAO_0000115>
        <oboInOwl:hasOBONamespace>GAZ</oboInOwl:hasOBONamespace>
        <oboInOwl:id>GAZ:00000672</oboInOwl:id>
        <rdfs:label>Al Jazirah State</rdfs:label>
    </owl:NamedIndividual>
    


    <!-- http://purl.obolibrary.org/obo/GAZ_00000673 -->

    <owl:NamedIndividual rdf:about="http://purl.obolibrary.org/obo/GAZ_00000673">
        <obo:RO_0001025 rdf:resource="http://purl.obolibrary.org/obo/GAZ_00233441"/>
        <obo:IAO_0000115>One of the states of Sudan.</obo:IAO_0000115>
        <oboInOwl:hasOBONamespace>GAZ</oboInOwl:hasOBONamespace>
        <oboInOwl:id>GAZ:00000673</oboInOwl:id>
        <rdfs:label>Al Qadarif State</rdfs:label>
    </owl:NamedIndividual>
    


    <!-- http://purl.obolibrary.org/obo/GAZ_00000674 -->

    <owl:NamedIndividual rdf:about="http://purl.obolibrary.org/obo/GAZ_00000674">
        <obo:RO_0001025 rdf:resource="http://purl.obolibrary.org/obo/GAZ_00233441"/>
        <obo:IAO_0000115>One of the states of Sudan.</obo:IAO_0000115>
        <oboInOwl:hasOBONamespace>GAZ</oboInOwl:hasOBONamespace>
        <oboInOwl:id>GAZ:00000674</oboInOwl:id>
        <rdfs:label>Blue Nile State</rdfs:label>
    </owl:NamedIndividual>
    


    <!-- http://purl.obolibrary.org/obo/GAZ_00000678 -->

    <owl:NamedIndividual rdf:about="http://purl.obolibrary.org/obo/GAZ_00000678">
        <obo:RO_0001025 rdf:resource="http://purl.obolibrary.org/obo/GAZ_00233441"/>
        <obo:IAO_0000115>One of the states of Sudan.</obo:IAO_0000115>
        <oboInOwl:hasOBONamespace>GAZ</oboInOwl:hasOBONamespace>
        <oboInOwl:id>GAZ:00000678</oboInOwl:id>
        <rdfs:label>Kassala State</rdfs:label>
    </owl:NamedIndividual>
    


    <!-- http://purl.obolibrary.org/obo/GAZ_00000679 -->

    <owl:NamedIndividual rdf:about="http://purl.obolibrary.org/obo/GAZ_00000679">
        <obo:RO_0001025 rdf:resource="http://purl.obolibrary.org/obo/GAZ_00233441"/>
        <obo:IAO_0000115>One of the states of Sudan.</obo:IAO_0000115>
        <oboInOwl:hasOBONamespace>GAZ</oboInOwl:hasOBONamespace>
        <oboInOwl:id>GAZ:00000679</oboInOwl:id>
        <rdfs:label>Khartoum State</rdfs:label>
    </owl:NamedIndividual>
    


    <!-- http://purl.obolibrary.org/obo/GAZ_00000682 -->

    <owl:NamedIndividual rdf:about="http://purl.obolibrary.org/obo/GAZ_00000682">
        <obo:RO_0001025 rdf:resource="http://purl.obolibrary.org/obo/GAZ_00004036"/>
        <obo:IAO_0000115>One of the states of Sudan.</obo:IAO_0000115>
        <oboInOwl:hasOBONamespace>GAZ</oboInOwl:hasOBONamespace>
        <oboInOwl:id>GAZ:00000682</oboInOwl:id>
        <rdfs:label>North Darfur State</rdfs:label>
    </owl:NamedIndividual>
    


    <!-- http://purl.obolibrary.org/obo/GAZ_00000683 -->

    <owl:NamedIndividual rdf:about="http://purl.obolibrary.org/obo/GAZ_00000683">
        <obo:RO_0001025 rdf:resource="http://purl.obolibrary.org/obo/GAZ_00233441"/>
        <obo:IAO_0000115>One of the states of Sudan.</obo:IAO_0000115>
        <oboInOwl:hasOBONamespace>GAZ</oboInOwl:hasOBONamespace>
        <oboInOwl:id>GAZ:00000683</oboInOwl:id>
        <rdfs:label>North Kurdufan State</rdfs:label>
    </owl:NamedIndividual>
    


    <!-- http://purl.obolibrary.org/obo/GAZ_00000684 -->

    <owl:NamedIndividual rdf:about="http://purl.obolibrary.org/obo/GAZ_00000684">
        <obo:RO_0001025 rdf:resource="http://purl.obolibrary.org/obo/GAZ_00233441"/>
        <obo:IAO_0000115>One of the 26 wilayat or states of Sudan.</obo:IAO_0000115>
        <oboInOwl:hasOBONamespace>GAZ</oboInOwl:hasOBONamespace>
        <oboInOwl:id>GAZ:00000684</oboInOwl:id>
        <rdfs:label>Northern State</rdfs:label>
    </owl:NamedIndividual>
    


    <!-- http://purl.obolibrary.org/obo/GAZ_00000685 -->

    <owl:NamedIndividual rdf:about="http://purl.obolibrary.org/obo/GAZ_00000685">
        <obo:RO_0001025 rdf:resource="http://purl.obolibrary.org/obo/GAZ_00233441"/>
        <obo:IAO_0000115>One of the states of Sudan.</obo:IAO_0000115>
        <oboInOwl:hasOBONamespace>GAZ</oboInOwl:hasOBONamespace>
        <oboInOwl:id>GAZ:00000685</oboInOwl:id>
        <rdfs:label>Red Sea State</rdfs:label>
    </owl:NamedIndividual>
    


    <!-- http://purl.obolibrary.org/obo/GAZ_00000686 -->

    <owl:NamedIndividual rdf:about="http://purl.obolibrary.org/obo/GAZ_00000686">
        <obo:RO_0001025 rdf:resource="http://purl.obolibrary.org/obo/GAZ_00233441"/>
        <obo:IAO_0000115>One of the states of Sudan.</obo:IAO_0000115>
        <oboInOwl:hasOBONamespace>GAZ</oboInOwl:hasOBONamespace>
        <oboInOwl:id>GAZ:00000686</oboInOwl:id>
        <rdfs:label>River Nile State</rdfs:label>
    </owl:NamedIndividual>
    


    <!-- http://purl.obolibrary.org/obo/GAZ_00000687 -->

    <owl:NamedIndividual rdf:about="http://purl.obolibrary.org/obo/GAZ_00000687">
        <obo:RO_0001025 rdf:resource="http://purl.obolibrary.org/obo/GAZ_00233441"/>
        <obo:IAO_0000115>One of the states of Sudan.</obo:IAO_0000115>
        <oboInOwl:hasOBONamespace>GAZ</oboInOwl:hasOBONamespace>
        <oboInOwl:id>GAZ:00000687</oboInOwl:id>
        <rdfs:label>Sennar State</rdfs:label>
    </owl:NamedIndividual>
    


    <!-- http://purl.obolibrary.org/obo/GAZ_00000688 -->

    <owl:NamedIndividual rdf:about="http://purl.obolibrary.org/obo/GAZ_00000688">
        <obo:RO_0001025 rdf:resource="http://purl.obolibrary.org/obo/GAZ_00004036"/>
        <obo:IAO_0000115>One of the states of Sudan.</obo:IAO_0000115>
        <oboInOwl:hasOBONamespace>GAZ</oboInOwl:hasOBONamespace>
        <oboInOwl:id>GAZ:00000688</oboInOwl:id>
        <rdfs:label>South Darfur State</rdfs:label>
    </owl:NamedIndividual>
    


    <!-- http://purl.obolibrary.org/obo/GAZ_00000689 -->

    <owl:NamedIndividual rdf:about="http://purl.obolibrary.org/obo/GAZ_00000689">
        <obo:RO_0001025 rdf:resource="http://purl.obolibrary.org/obo/GAZ_00233441"/>
        <obo:IAO_0000115>One of the states of Sudan.</obo:IAO_0000115>
        <oboInOwl:hasOBONamespace>GAZ</oboInOwl:hasOBONamespace>
        <oboInOwl:id>GAZ:00000689</oboInOwl:id>
        <rdfs:label>South Kurdufan State</rdfs:label>
    </owl:NamedIndividual>
    


    <!-- http://purl.obolibrary.org/obo/GAZ_00000694 -->

    <owl:NamedIndividual rdf:about="http://purl.obolibrary.org/obo/GAZ_00000694">
        <obo:RO_0001025 rdf:resource="http://purl.obolibrary.org/obo/GAZ_00004036"/>
        <obo:IAO_0000115>One of the states of Sudan.</obo:IAO_0000115>
        <oboInOwl:hasOBONamespace>GAZ</oboInOwl:hasOBONamespace>
        <oboInOwl:id>GAZ:00000694</oboInOwl:id>
        <rdfs:label>West Darfur State</rdfs:label>
    </owl:NamedIndividual>
    


    <!-- http://purl.obolibrary.org/obo/GAZ_00000696 -->

    <owl:NamedIndividual rdf:about="http://purl.obolibrary.org/obo/GAZ_00000696">
        <obo:RO_0001025 rdf:resource="http://purl.obolibrary.org/obo/GAZ_00233441"/>
        <obo:IAO_0000115>One of the states of Sudan.</obo:IAO_0000115>
        <oboInOwl:hasOBONamespace>GAZ</oboInOwl:hasOBONamespace>
        <oboInOwl:id>GAZ:00000696</oboInOwl:id>
        <rdfs:label>White Nile State</rdfs:label>
    </owl:NamedIndividual>
    


    <!-- http://purl.obolibrary.org/obo/GAZ_00002456 -->

    <owl:NamedIndividual rdf:about="http://purl.obolibrary.org/obo/GAZ_00002456">
        <obo:RO_0001025 rdf:resource="http://purl.obolibrary.org/obo/GAZ_00000685"/>
        <obo:IAO_0000115>A sea situated between the coasts of Africa and the Arabian Peninsula, are the following: On the North: A line joining the coast of Africa, in Egypt, eastward, along the parallel of 27 Degrees 27 Minutes N, to the southern extremity of Shaker Island (27 Degrees 27 Minutes N - 34 Degrees 02 Minutes 10 Seconds E), and northeastward to Cape Muhammad (27 Degrees 43 Minutes 35 Seconds N - 34 Degrees 15 Minutes E), the southern extremity of the Sinai Peninsula (the common limit with the Gulf of Suez); thence from Cape Muhammad northeastward, along the southern coast of the Sinai Peninsula, to the parallel of 27 Degrees 54 Minutes 50 Seconds N; thence a line joining the southern coast of the Sinai Peninsula eastward, along the parallel of 27 Degrees 54 Minutes 50 Seconds N, to the southwestern extremity of T Degrees r Degrees n Island (27 Degrees 54 Minutes 50 Seconds N - 34 Degrees 33 Minutes E); thence from the southwestern extremity of T Degrees r Degrees n Island northward, through this island, to position 27 Degrees 58 Minutes 10 Seconds N - 34 Degrees 35 Minutes E), on the northeastern coast thereof; and thence a line joining this position northeastward to Cape Al Qa Degrees bah (28 Degrees 01 Minutes 30 Seconds N - 34 Degrees 37 Minutes 15 Seconds E), in Saudi Arabia (the common limit with the Gulf of Aqaba). On the East: From Cape Al Qa Degrees bah, in Saudi Arabia, southeastward, along the coast of the Arabian Peninsula, to Hisn Mur Degrees d (12 Degrees 40 Minutes 20 Seconds N - 43 Degrees 30 Minutes 20 Seconds E), in Southern Yemen. On the South: A line joining Hisn Mur Degrees d, in Southern Yemen, southwestward to Cape Si Ane (12 Degrees 28 Minutes 50 Seconds N - 43 Degrees 19 Minutes 10 Seconds E), in Djibouti (the common limit with the Gulf of Aden). On the West: From Cape Si Ane, in Djibouti, northwestward, along the coast of Africa, to the parallel of 27 Degrees 27 Minutes N, in Egypt.</obo:IAO_0000115>
        <oboInOwl:hasOBONamespace>GAZ</oboInOwl:hasOBONamespace>
        <oboInOwl:id>GAZ:00002456</oboInOwl:id>
        <rdfs:label>Red Sea</rdfs:label>
    </owl:NamedIndividual>
    


    <!-- http://purl.obolibrary.org/obo/GAZ_00004033 -->

    <owl:NamedIndividual rdf:about="http://purl.obolibrary.org/obo/GAZ_00004033">
        <oboInOwl:hasOBONamespace>GAZ</oboInOwl:hasOBONamespace>
        <oboInOwl:id>GAZ:00004033</oboInOwl:id>
        <rdfs:label>Northern Sahara Desert</rdfs:label>
    </owl:NamedIndividual>
    


    <!-- http://purl.obolibrary.org/obo/GAZ_00004036 -->

    <owl:NamedIndividual rdf:about="http://purl.obolibrary.org/obo/GAZ_00004036">
        <obo:RO_0001025 rdf:resource="http://purl.obolibrary.org/obo/GAZ_00000560"/>
        <obo:IAO_0000115>A region of far western Sudan, bordering the Central African Republic, Libya, and Chad. It is divided into three federal states within Sudan: Gharb Darfur (West Darfur), Janub Darfur (South Darfur), and Shamal Darfur (North Darfur).</obo:IAO_0000115>
        <oboInOwl:hasOBONamespace>GAZ</oboInOwl:hasOBONamespace>
        <oboInOwl:id>GAZ:00004036</oboInOwl:id>
        <rdfs:label>Darfur</rdfs:label>
    </owl:NamedIndividual>
    


    <!-- http://purl.obolibrary.org/obo/GAZ_00004037 -->

    <owl:NamedIndividual rdf:about="http://purl.obolibrary.org/obo/GAZ_00004037">
        <obo:RO_0001025 rdf:resource="http://purl.obolibrary.org/obo/GAZ_00144637"/>
        <obo:IAO_0000115>A small shore island in the Red Sea. It is owned by Egypt and can be found at the northern entrance to Foul Bay.</obo:IAO_0000115>
        <oboInOwl:hasOBONamespace>GAZ</oboInOwl:hasOBONamespace>
        <oboInOwl:id>GAZ:00004037</oboInOwl:id>
        <rdfs:label>Mukawwar Island</rdfs:label>
    </owl:NamedIndividual>
    


    <!-- http://purl.obolibrary.org/obo/GAZ_00005876 -->

    <owl:NamedIndividual rdf:about="http://purl.obolibrary.org/obo/GAZ_00005876">
        <rdf:type rdf:resource="http://purl.obolibrary.org/obo/ENVO_00000220"/>
        <obo:RO_0001025 rdf:resource="http://purl.obolibrary.org/obo/GAZ_00053597"/>
        <obo:IAO_0000115>An island group in the Red Sea. Most of them are a part of Yemen, but before 1998-1999 they were claimed by Eritrea as well. They are formed from a series of volcanic vents along a NE-SW trend, and include the Holocene Great Hanish, Little Hanish, and many other small islands and submarine shoals.</obo:IAO_0000115>
        <oboInOwl:hasOBONamespace>GAZ</oboInOwl:hasOBONamespace>
        <oboInOwl:id>GAZ:00005876</oboInOwl:id>
        <rdfs:label>Hanish Islands</rdfs:label>
    </owl:NamedIndividual>
    


    <!-- http://purl.obolibrary.org/obo/GAZ_00005877 -->

    <owl:NamedIndividual rdf:about="http://purl.obolibrary.org/obo/GAZ_00005877">
        <obo:RO_0001025 rdf:resource="http://purl.obolibrary.org/obo/GAZ_00002456"/>
        <obo:IAO_0000115>A &quot;shelf island&quot; located in the shallow waters of the Arabian peninsula&apos;s continental shelf with coral reefs surrounding three sides of the island.</obo:IAO_0000115>
        <oboInOwl:hasOBONamespace>GAZ</oboInOwl:hasOBONamespace>
        <oboInOwl:id>GAZ:00005877</oboInOwl:id>
        <rdfs:label>Kamaran Island</rdfs:label>
    </owl:NamedIndividual>
    


    <!-- http://purl.obolibrary.org/obo/GAZ_00005878 -->

    <owl:NamedIndividual rdf:about="http://purl.obolibrary.org/obo/GAZ_00005878">
        <rdf:type rdf:resource="http://purl.obolibrary.org/obo/ENVO_00000222"/>
        <obo:RO_0001025 rdf:resource="http://purl.obolibrary.org/obo/GAZ_00051269"/>
        <obo:IAO_0000115>A volcanic island located in the Strait of Mandeb at the southern entrance into the Red Sea off the southwestern coast of Yemen.</obo:IAO_0000115>
        <oboInOwl:hasOBONamespace>GAZ</oboInOwl:hasOBONamespace>
        <oboInOwl:id>GAZ:00005878</oboInOwl:id>
        <rdfs:label>Perim</rdfs:label>
    </owl:NamedIndividual>
    


    <!-- http://purl.obolibrary.org/obo/GAZ_00005879 -->

    <owl:NamedIndividual rdf:about="http://purl.obolibrary.org/obo/GAZ_00005879">
        <obo:RO_0001025 rdf:resource="http://purl.obolibrary.org/obo/GAZ_00053597"/>
        <obo:IAO_0000115>An island of Yemen in the Red Sea. It lies the coasts of Yemen and Eritrea near the Bab-el-Mandeb straits, which connect the Red Sea to the Gulf of Aden. Despite its proximity to the African continent, it is considered an island of Asia because it sits on the Asian continental shelf. A shield volcano.</obo:IAO_0000115>
        <oboInOwl:hasOBONamespace>GAZ</oboInOwl:hasOBONamespace>
        <oboInOwl:id>GAZ:00005879</oboInOwl:id>
        <rdfs:label>Zuqar Island</rdfs:label>
    </owl:NamedIndividual>
    


    <!-- http://purl.obolibrary.org/obo/GAZ_00007859 -->

    <owl:NamedIndividual rdf:about="http://purl.obolibrary.org/obo/GAZ_00007859">
        <obo:RO_0001025 rdf:resource="http://purl.obolibrary.org/obo/GAZ_00000560"/>
    </owl:NamedIndividual>
    


    <!-- http://purl.obolibrary.org/obo/GAZ_00007860 -->

    <owl:NamedIndividual rdf:about="http://purl.obolibrary.org/obo/GAZ_00007860">
        <obo:RO_0001025 rdf:resource="http://purl.obolibrary.org/obo/GAZ_00032221"/>
    </owl:NamedIndividual>
    


    <!-- http://purl.obolibrary.org/obo/GAZ_00008153 -->

    <owl:NamedIndividual rdf:about="http://purl.obolibrary.org/obo/GAZ_00008153">
        <rdf:type rdf:resource="http://purl.obolibrary.org/obo/ENVO_00000033"/>
        <obo:RO_0001025 rdf:resource="http://purl.obolibrary.org/obo/GAZ_00002456"/>
        <obo:IAO_0000115>A submarine basin. A pool of hot saline brine at the bottom of the central rift in the Red Sea.</obo:IAO_0000115>
        <oboInOwl:hasOBONamespace>GAZ</oboInOwl:hasOBONamespace>
        <oboInOwl:id>GAZ:00008153</oboInOwl:id>
        <rdfs:label>Atlantis II Deep</rdfs:label>
    </owl:NamedIndividual>
    


    <!-- http://purl.obolibrary.org/obo/GAZ_00008589 -->

    <owl:NamedIndividual rdf:about="http://purl.obolibrary.org/obo/GAZ_00008589">
        <obo:RO_0001025 rdf:resource="http://purl.obolibrary.org/obo/GAZ_00000678"/>
        <obo:IAO_0000115>A populated place.</obo:IAO_0000115>
        <oboInOwl:hasOBONamespace>GAZ</oboInOwl:hasOBONamespace>
        <oboInOwl:id>GAZ:00008589</oboInOwl:id>
        <rdfs:label>El Fau</rdfs:label>
    </owl:NamedIndividual>
    


    <!-- http://purl.obolibrary.org/obo/GAZ_00009408 -->

    <owl:NamedIndividual rdf:about="http://purl.obolibrary.org/obo/GAZ_00009408">
        <obo:RO_0001025 rdf:resource="http://purl.obolibrary.org/obo/GAZ_00000685"/>
        <obo:RO_0001025 rdf:resource="http://purl.obolibrary.org/obo/GAZ_00002456"/>
        <oboInOwl:hasOBONamespace>GAZ</oboInOwl:hasOBONamespace>
        <oboInOwl:id>GAZ:00009408</oboInOwl:id>
        <rdfs:label>Suakin Archipelago</rdfs:label>
    </owl:NamedIndividual>
    


    <!-- http://purl.obolibrary.org/obo/GAZ_00009683 -->

    <owl:NamedIndividual rdf:about="http://purl.obolibrary.org/obo/GAZ_00009683">
        <rdf:type rdf:resource="http://purl.obolibrary.org/obo/ENVO_00000220"/>
        <obo:RO_0001025 rdf:resource="http://purl.obolibrary.org/obo/GAZ_00002456"/>
        <obo:IAO_0000115>An island group located in the Red Sea near Massawa, Eritrea. It consists of two large and 124 small islands.</obo:IAO_0000115>
        <oboInOwl:hasOBONamespace>GAZ</oboInOwl:hasOBONamespace>
        <oboInOwl:id>GAZ:00009683</oboInOwl:id>
        <rdfs:label>Dahlak Archipelago</rdfs:label>
    </owl:NamedIndividual>
    


    <!-- http://purl.obolibrary.org/obo/GAZ_00009949 -->

    <owl:NamedIndividual rdf:about="http://purl.obolibrary.org/obo/GAZ_00009949">
        <obo:IAO_0000115>The delta formed in Northern Egypt where the Nile River spreads out and drains into the Mediterranean Sea. It is one of the world&apos;s largest river delta, from Alexandria in the west to Port Said in the east, it covers some 240 km of Mediterranean coastline.</obo:IAO_0000115>
        <oboInOwl:hasOBONamespace>GAZ</oboInOwl:hasOBONamespace>
        <oboInOwl:id>GAZ:00009949</oboInOwl:id>
        <rdfs:label>Nile Delta</rdfs:label>
    </owl:NamedIndividual>
    


    <!-- http://purl.obolibrary.org/obo/GAZ_00031012 -->

    <owl:NamedIndividual rdf:about="http://purl.obolibrary.org/obo/GAZ_00031012">
        <obo:RO_0001025 rdf:resource="http://purl.obolibrary.org/obo/GAZ_00051197"/>
        <obo:IAO_0000115>One of the seven oases of the Western Desert of Egypt (part of the Libyan Desert). Dakhla Oasis is located at 350 km from the Nile Valley and is also situated between the oases of Farafra and Kharga. It measures some 80 km from east to west and about 25 km from north to south.</obo:IAO_0000115>
        <oboInOwl:hasOBONamespace>GAZ</oboInOwl:hasOBONamespace>
        <oboInOwl:id>GAZ:00031012</oboInOwl:id>
        <rdfs:label>Dakhla Oasis</rdfs:label>
    </owl:NamedIndividual>
    


    <!-- http://purl.obolibrary.org/obo/GAZ_00031013 -->

    <owl:NamedIndividual rdf:about="http://purl.obolibrary.org/obo/GAZ_00031013">
        <obo:RO_0001025 rdf:resource="http://purl.obolibrary.org/obo/GAZ_00051197"/>
        <obo:IAO_0000115>The southernmost of Egypt&apos;s five western oases. It is located in the Libyan Desert, about 200 km to the west of the Nile valley, and is some 150 km long. It is located in and is the capital of El Wadi el Gedid governorate.</obo:IAO_0000115>
        <oboInOwl:hasOBONamespace>GAZ</oboInOwl:hasOBONamespace>
        <oboInOwl:id>GAZ:00031013</oboInOwl:id>
        <rdfs:label>Kharga Oasis</rdfs:label>
    </owl:NamedIndividual>
    


    <!-- http://purl.obolibrary.org/obo/GAZ_00031014 -->

    <owl:NamedIndividual rdf:about="http://purl.obolibrary.org/obo/GAZ_00031014">
        <obo:RO_0001025 rdf:resource="http://purl.obolibrary.org/obo/GAZ_00051197"/>
        <oboInOwl:hasOBONamespace>GAZ</oboInOwl:hasOBONamespace>
        <oboInOwl:id>GAZ:00031014</oboInOwl:id>
        <rdfs:label>Baris Oasis</rdfs:label>
    </owl:NamedIndividual>
    


    <!-- http://purl.obolibrary.org/obo/GAZ_00031015 -->

    <owl:NamedIndividual rdf:about="http://purl.obolibrary.org/obo/GAZ_00031015">
        <obo:RO_0001025 rdf:resource="http://purl.obolibrary.org/obo/GAZ_00051197"/>
        <obo:IAO_0000115>The smallest oasis located in Western Egypt. It is located in the Libyan Desert, approximately mid-way between Dakhla and Bahariya.</obo:IAO_0000115>
        <oboInOwl:hasOBONamespace>GAZ</oboInOwl:hasOBONamespace>
        <oboInOwl:id>GAZ:00031015</oboInOwl:id>
        <rdfs:label>Farafra Oasis</rdfs:label>
    </owl:NamedIndividual>
    


    <!-- http://purl.obolibrary.org/obo/GAZ_00032220 -->

    <owl:NamedIndividual rdf:about="http://purl.obolibrary.org/obo/GAZ_00032220">
        <rdf:type rdf:resource="http://purl.obolibrary.org/obo/ENVO_00000004"/>
        <obo:RO_0001025 rdf:resource="http://purl.obolibrary.org/obo/GAZ_00000696"/>
        <obo:IAO_0000115>A district of White Nile State.</obo:IAO_0000115>
        <oboInOwl:hasOBONamespace>GAZ</oboInOwl:hasOBONamespace>
        <oboInOwl:id>GAZ:00032220</oboInOwl:id>
        <rdfs:label>Ad Douiem District</rdfs:label>
    </owl:NamedIndividual>
    


    <!-- http://purl.obolibrary.org/obo/GAZ_00032221 -->

    <owl:NamedIndividual rdf:about="http://purl.obolibrary.org/obo/GAZ_00032221">
        <rdf:type rdf:resource="http://purl.obolibrary.org/obo/ENVO_00000004"/>
        <obo:RO_0001025 rdf:resource="http://purl.obolibrary.org/obo/GAZ_00000696"/>
        <obo:IAO_0000115>A district of White Nile State.</obo:IAO_0000115>
        <oboInOwl:hasOBONamespace>GAZ</oboInOwl:hasOBONamespace>
        <oboInOwl:id>GAZ:00032221</oboInOwl:id>
        <rdfs:label>Kosti District</rdfs:label>
    </owl:NamedIndividual>
    


    <!-- http://purl.obolibrary.org/obo/GAZ_00032222 -->

    <owl:NamedIndividual rdf:about="http://purl.obolibrary.org/obo/GAZ_00032222">
        <rdf:type rdf:resource="http://purl.obolibrary.org/obo/ENVO_00000004"/>
        <obo:RO_0001025 rdf:resource="http://purl.obolibrary.org/obo/GAZ_00000696"/>
        <obo:IAO_0000115>A district of White Nile State.</obo:IAO_0000115>
        <oboInOwl:hasOBONamespace>GAZ</oboInOwl:hasOBONamespace>
        <oboInOwl:id>GAZ:00032222</oboInOwl:id>
        <rdfs:label>Al Jabalian District</rdfs:label>
    </owl:NamedIndividual>
    


    <!-- http://purl.obolibrary.org/obo/GAZ_00032223 -->

    <owl:NamedIndividual rdf:about="http://purl.obolibrary.org/obo/GAZ_00032223">
        <rdf:type rdf:resource="http://purl.obolibrary.org/obo/ENVO_00000004"/>
        <obo:RO_0001025 rdf:resource="http://purl.obolibrary.org/obo/GAZ_00000696"/>
        <obo:IAO_0000115>A district of White Nile State.</obo:IAO_0000115>
        <oboInOwl:hasOBONamespace>GAZ</oboInOwl:hasOBONamespace>
        <oboInOwl:id>GAZ:00032223</oboInOwl:id>
        <rdfs:label>Al Gutaina District</rdfs:label>
    </owl:NamedIndividual>
    


    <!-- http://purl.obolibrary.org/obo/GAZ_00032224 -->

    <owl:NamedIndividual rdf:about="http://purl.obolibrary.org/obo/GAZ_00032224">
        <rdf:type rdf:resource="http://purl.obolibrary.org/obo/ENVO_00000004"/>
        <obo:RO_0001025 rdf:resource="http://purl.obolibrary.org/obo/GAZ_00000689"/>
        <obo:IAO_0000115>A district of South Kurdufan State.</obo:IAO_0000115>
        <oboInOwl:hasOBONamespace>GAZ</oboInOwl:hasOBONamespace>
        <oboInOwl:id>GAZ:00032224</oboInOwl:id>
        <rdfs:label>Lagawa District</rdfs:label>
    </owl:NamedIndividual>
    


    <!-- http://purl.obolibrary.org/obo/GAZ_00032225 -->

    <owl:NamedIndividual rdf:about="http://purl.obolibrary.org/obo/GAZ_00032225">
        <rdf:type rdf:resource="http://purl.obolibrary.org/obo/ENVO_00000004"/>
        <obo:RO_0001025 rdf:resource="http://purl.obolibrary.org/obo/GAZ_00000689"/>
        <obo:IAO_0000115>A district of South Kurdufan State. The area is claimed by South Sudan but currently controlled by the northern Sudanese government.</obo:IAO_0000115>
        <oboInOwl:hasOBONamespace>GAZ</oboInOwl:hasOBONamespace>
        <oboInOwl:id>GAZ:00032225</oboInOwl:id>
        <rdfs:label>Abyei District</rdfs:label>
    </owl:NamedIndividual>
    


    <!-- http://purl.obolibrary.org/obo/GAZ_00032226 -->

    <owl:NamedIndividual rdf:about="http://purl.obolibrary.org/obo/GAZ_00032226">
        <rdf:type rdf:resource="http://purl.obolibrary.org/obo/ENVO_00000004"/>
        <obo:RO_0001025 rdf:resource="http://purl.obolibrary.org/obo/GAZ_00000683"/>
        <obo:IAO_0000115>A district of North Kurdufan State.</obo:IAO_0000115>
        <oboInOwl:hasOBONamespace>GAZ</oboInOwl:hasOBONamespace>
        <oboInOwl:id>GAZ:00032226</oboInOwl:id>
        <rdfs:label>Ghebeish District</rdfs:label>
    </owl:NamedIndividual>
    


    <!-- http://purl.obolibrary.org/obo/GAZ_00032227 -->

    <owl:NamedIndividual rdf:about="http://purl.obolibrary.org/obo/GAZ_00032227">
        <rdf:type rdf:resource="http://purl.obolibrary.org/obo/ENVO_00000004"/>
        <obo:RO_0001025 rdf:resource="http://purl.obolibrary.org/obo/GAZ_00000683"/>
        <obo:IAO_0000115>A district of North Kurdufan State.</obo:IAO_0000115>
        <oboInOwl:hasOBONamespace>GAZ</oboInOwl:hasOBONamespace>
        <oboInOwl:id>GAZ:00032227</oboInOwl:id>
        <rdfs:label>En Nuhud District</rdfs:label>
    </owl:NamedIndividual>
    


    <!-- http://purl.obolibrary.org/obo/GAZ_00032228 -->

    <owl:NamedIndividual rdf:about="http://purl.obolibrary.org/obo/GAZ_00032228">
        <rdf:type rdf:resource="http://purl.obolibrary.org/obo/ENVO_00000004"/>
        <obo:RO_0001025 rdf:resource="http://purl.obolibrary.org/obo/GAZ_00000683"/>
        <obo:IAO_0000115>A district of North Kurdufan State.</obo:IAO_0000115>
        <oboInOwl:hasOBONamespace>GAZ</oboInOwl:hasOBONamespace>
        <oboInOwl:id>GAZ:00032228</oboInOwl:id>
        <rdfs:label>As Salam District</rdfs:label>
    </owl:NamedIndividual>
    


    <!-- http://purl.obolibrary.org/obo/GAZ_00032229 -->

    <owl:NamedIndividual rdf:about="http://purl.obolibrary.org/obo/GAZ_00032229">
        <rdf:type rdf:resource="http://purl.obolibrary.org/obo/ENVO_00000004"/>
        <obo:RO_0001025 rdf:resource="http://purl.obolibrary.org/obo/GAZ_00000694"/>
        <obo:IAO_0000115>A district of West Dafur State.</obo:IAO_0000115>
        <oboInOwl:hasOBONamespace>GAZ</oboInOwl:hasOBONamespace>
        <oboInOwl:id>GAZ:00032229</oboInOwl:id>
        <rdfs:label>Habillah District</rdfs:label>
    </owl:NamedIndividual>
    


    <!-- http://purl.obolibrary.org/obo/GAZ_00032230 -->

    <owl:NamedIndividual rdf:about="http://purl.obolibrary.org/obo/GAZ_00032230">
        <rdf:type rdf:resource="http://purl.obolibrary.org/obo/ENVO_00000004"/>
        <obo:RO_0001025 rdf:resource="http://purl.obolibrary.org/obo/GAZ_00000694"/>
        <obo:IAO_0000115>A district of West Dafur State.</obo:IAO_0000115>
        <oboInOwl:hasOBONamespace>GAZ</oboInOwl:hasOBONamespace>
        <oboInOwl:id>GAZ:00032230</oboInOwl:id>
        <rdfs:label>Jebel Marra District</rdfs:label>
    </owl:NamedIndividual>
    


    <!-- http://purl.obolibrary.org/obo/GAZ_00032231 -->

    <owl:NamedIndividual rdf:about="http://purl.obolibrary.org/obo/GAZ_00032231">
        <rdf:type rdf:resource="http://purl.obolibrary.org/obo/ENVO_00000004"/>
        <obo:RO_0001025 rdf:resource="http://purl.obolibrary.org/obo/GAZ_00000694"/>
        <obo:IAO_0000115>A district of West Dafur State.</obo:IAO_0000115>
        <oboInOwl:hasOBONamespace>GAZ</oboInOwl:hasOBONamespace>
        <oboInOwl:id>GAZ:00032231</oboInOwl:id>
        <rdfs:label>Mukjar District</rdfs:label>
    </owl:NamedIndividual>
    


    <!-- http://purl.obolibrary.org/obo/GAZ_00032232 -->

    <owl:NamedIndividual rdf:about="http://purl.obolibrary.org/obo/GAZ_00032232">
        <rdf:type rdf:resource="http://purl.obolibrary.org/obo/ENVO_00000004"/>
        <obo:RO_0001025 rdf:resource="http://purl.obolibrary.org/obo/GAZ_00000694"/>
        <obo:IAO_0000115>A district of West Dafur State.</obo:IAO_0000115>
        <oboInOwl:hasOBONamespace>GAZ</oboInOwl:hasOBONamespace>
        <oboInOwl:id>GAZ:00032232</oboInOwl:id>
        <rdfs:label>Wadi Salih District</rdfs:label>
    </owl:NamedIndividual>
    


    <!-- http://purl.obolibrary.org/obo/GAZ_00032233 -->

    <owl:NamedIndividual rdf:about="http://purl.obolibrary.org/obo/GAZ_00032233">
        <rdf:type rdf:resource="http://purl.obolibrary.org/obo/ENVO_00000004"/>
        <obo:RO_0001025 rdf:resource="http://purl.obolibrary.org/obo/GAZ_00000694"/>
        <obo:IAO_0000115>A district of West Dafur State.</obo:IAO_0000115>
        <oboInOwl:hasOBONamespace>GAZ</oboInOwl:hasOBONamespace>
        <oboInOwl:id>GAZ:00032233</oboInOwl:id>
        <rdfs:label>Al Geneina District</rdfs:label>
    </owl:NamedIndividual>
    


    <!-- http://purl.obolibrary.org/obo/GAZ_00032234 -->

    <owl:NamedIndividual rdf:about="http://purl.obolibrary.org/obo/GAZ_00032234">
        <obo:RO_0001025 rdf:resource="http://purl.obolibrary.org/obo/GAZ_00000694"/>
        <oboInOwl:hasOBONamespace>GAZ</oboInOwl:hasOBONamespace>
        <oboInOwl:id>GAZ:00032234</oboInOwl:id>
        <rdfs:label>Kulbus District</rdfs:label>
    </owl:NamedIndividual>
    


    <!-- http://purl.obolibrary.org/obo/GAZ_00032235 -->

    <owl:NamedIndividual rdf:about="http://purl.obolibrary.org/obo/GAZ_00032235">
        <obo:RO_0001025 rdf:resource="http://purl.obolibrary.org/obo/GAZ_00000694"/>
        <oboInOwl:hasOBONamespace>GAZ</oboInOwl:hasOBONamespace>
        <oboInOwl:id>GAZ:00032235</oboInOwl:id>
        <rdfs:label>Zallingi District</rdfs:label>
    </owl:NamedIndividual>
    


    <!-- http://purl.obolibrary.org/obo/GAZ_00032255 -->

    <owl:NamedIndividual rdf:about="http://purl.obolibrary.org/obo/GAZ_00032255">
        <rdf:type rdf:resource="http://purl.obolibrary.org/obo/ENVO_00000004"/>
        <obo:RO_0001025 rdf:resource="http://purl.obolibrary.org/obo/GAZ_00000689"/>
        <obo:IAO_0000115>A district of South Kurdufan State.</obo:IAO_0000115>
        <oboInOwl:hasOBONamespace>GAZ</oboInOwl:hasOBONamespace>
        <oboInOwl:id>GAZ:00032255</oboInOwl:id>
        <rdfs:label>Dilling District</rdfs:label>
    </owl:NamedIndividual>
    


    <!-- http://purl.obolibrary.org/obo/GAZ_00032256 -->

    <owl:NamedIndividual rdf:about="http://purl.obolibrary.org/obo/GAZ_00032256">
        <rdf:type rdf:resource="http://purl.obolibrary.org/obo/ENVO_00000004"/>
        <obo:RO_0001025 rdf:resource="http://purl.obolibrary.org/obo/GAZ_00000688"/>
        <obo:IAO_0000115>A district of South Dafur State.</obo:IAO_0000115>
        <oboInOwl:hasOBONamespace>GAZ</oboInOwl:hasOBONamespace>
        <oboInOwl:id>GAZ:00032256</oboInOwl:id>
        <rdfs:label>Nyala District</rdfs:label>
    </owl:NamedIndividual>
    


    <!-- http://purl.obolibrary.org/obo/GAZ_00032257 -->

    <owl:NamedIndividual rdf:about="http://purl.obolibrary.org/obo/GAZ_00032257">
        <rdf:type rdf:resource="http://purl.obolibrary.org/obo/ENVO_00000004"/>
        <obo:RO_0001025 rdf:resource="http://purl.obolibrary.org/obo/GAZ_00000689"/>
        <obo:IAO_0000115>A district of South Kurdufan State.</obo:IAO_0000115>
        <oboInOwl:hasOBONamespace>GAZ</oboInOwl:hasOBONamespace>
        <oboInOwl:id>GAZ:00032257</oboInOwl:id>
        <rdfs:label>Talodi District</rdfs:label>
    </owl:NamedIndividual>
    


    <!-- http://purl.obolibrary.org/obo/GAZ_00032258 -->

    <owl:NamedIndividual rdf:about="http://purl.obolibrary.org/obo/GAZ_00032258">
        <rdf:type rdf:resource="http://purl.obolibrary.org/obo/ENVO_00000004"/>
        <obo:RO_0001025 rdf:resource="http://purl.obolibrary.org/obo/GAZ_00000688"/>
        <obo:IAO_0000115>A district of South Dafur State.</obo:IAO_0000115>
        <oboInOwl:hasOBONamespace>GAZ</oboInOwl:hasOBONamespace>
        <oboInOwl:id>GAZ:00032258</oboInOwl:id>
        <rdfs:label>Kas District</rdfs:label>
    </owl:NamedIndividual>
    


    <!-- http://purl.obolibrary.org/obo/GAZ_00032259 -->

    <owl:NamedIndividual rdf:about="http://purl.obolibrary.org/obo/GAZ_00032259">
        <rdf:type rdf:resource="http://purl.obolibrary.org/obo/ENVO_00000004"/>
        <obo:RO_0001025 rdf:resource="http://purl.obolibrary.org/obo/GAZ_00000688"/>
        <obo:IAO_0000115>A district of South Dafur State.</obo:IAO_0000115>
        <oboInOwl:hasOBONamespace>GAZ</oboInOwl:hasOBONamespace>
        <oboInOwl:id>GAZ:00032259</oboInOwl:id>
        <rdfs:label>Adayala District</rdfs:label>
    </owl:NamedIndividual>
    


    <!-- http://purl.obolibrary.org/obo/GAZ_00032260 -->

    <owl:NamedIndividual rdf:about="http://purl.obolibrary.org/obo/GAZ_00032260">
        <rdf:type rdf:resource="http://purl.obolibrary.org/obo/ENVO_00000004"/>
        <obo:RO_0001025 rdf:resource="http://purl.obolibrary.org/obo/GAZ_00000688"/>
        <obo:IAO_0000115>A district of South Dafur State.</obo:IAO_0000115>
        <oboInOwl:hasOBONamespace>GAZ</oboInOwl:hasOBONamespace>
        <oboInOwl:id>GAZ:00032260</oboInOwl:id>
        <rdfs:label>Shearia District</rdfs:label>
    </owl:NamedIndividual>
    


    <!-- http://purl.obolibrary.org/obo/GAZ_00032261 -->

    <owl:NamedIndividual rdf:about="http://purl.obolibrary.org/obo/GAZ_00032261">
        <rdf:type rdf:resource="http://purl.obolibrary.org/obo/ENVO_00000004"/>
        <obo:RO_0001025 rdf:resource="http://purl.obolibrary.org/obo/GAZ_00000688"/>
        <obo:IAO_0000115>A district of South Dafur State.</obo:IAO_0000115>
        <oboInOwl:hasOBONamespace>GAZ</oboInOwl:hasOBONamespace>
        <oboInOwl:id>GAZ:00032261</oboInOwl:id>
        <rdfs:label>Buram District</rdfs:label>
    </owl:NamedIndividual>
    


    <!-- http://purl.obolibrary.org/obo/GAZ_00032262 -->

    <owl:NamedIndividual rdf:about="http://purl.obolibrary.org/obo/GAZ_00032262">
        <rdf:type rdf:resource="http://purl.obolibrary.org/obo/ENVO_00000004"/>
        <obo:RO_0001025 rdf:resource="http://purl.obolibrary.org/obo/GAZ_00000689"/>
        <obo:IAO_0000115>A district of South Kurdufan State.</obo:IAO_0000115>
        <oboInOwl:hasOBONamespace>GAZ</oboInOwl:hasOBONamespace>
        <oboInOwl:id>GAZ:00032262</oboInOwl:id>
        <rdfs:label>Abu Jubaiyah District</rdfs:label>
    </owl:NamedIndividual>
    


    <!-- http://purl.obolibrary.org/obo/GAZ_00032263 -->

    <owl:NamedIndividual rdf:about="http://purl.obolibrary.org/obo/GAZ_00032263">
        <rdf:type rdf:resource="http://purl.obolibrary.org/obo/ENVO_00000004"/>
        <obo:RO_0001025 rdf:resource="http://purl.obolibrary.org/obo/GAZ_00000689"/>
        <obo:IAO_0000115>A district of South Kurdufan State.</obo:IAO_0000115>
        <oboInOwl:hasOBONamespace>GAZ</oboInOwl:hasOBONamespace>
        <oboInOwl:id>GAZ:00032263</oboInOwl:id>
        <rdfs:label>Kadugli District</rdfs:label>
    </owl:NamedIndividual>
    


    <!-- http://purl.obolibrary.org/obo/GAZ_00032264 -->

    <owl:NamedIndividual rdf:about="http://purl.obolibrary.org/obo/GAZ_00032264">
        <rdf:type rdf:resource="http://purl.obolibrary.org/obo/ENVO_00000004"/>
        <obo:RO_0001025 rdf:resource="http://purl.obolibrary.org/obo/GAZ_00000689"/>
        <obo:IAO_0000115>A district of South Kurdufan State.</obo:IAO_0000115>
        <oboInOwl:hasOBONamespace>GAZ</oboInOwl:hasOBONamespace>
        <oboInOwl:id>GAZ:00032264</oboInOwl:id>
        <rdfs:label>Rashad District</rdfs:label>
    </owl:NamedIndividual>
    


    <!-- http://purl.obolibrary.org/obo/GAZ_00032265 -->

    <owl:NamedIndividual rdf:about="http://purl.obolibrary.org/obo/GAZ_00032265">
        <rdf:type rdf:resource="http://purl.obolibrary.org/obo/ENVO_00000004"/>
        <obo:RO_0001025 rdf:resource="http://purl.obolibrary.org/obo/GAZ_00000688"/>
        <obo:IAO_0000115>A district of South Dafur State.</obo:IAO_0000115>
        <oboInOwl:hasOBONamespace>GAZ</oboInOwl:hasOBONamespace>
        <oboInOwl:id>GAZ:00032265</oboInOwl:id>
        <rdfs:label>Edd al Fursan District</rdfs:label>
    </owl:NamedIndividual>
    


    <!-- http://purl.obolibrary.org/obo/GAZ_00032266 -->

    <owl:NamedIndividual rdf:about="http://purl.obolibrary.org/obo/GAZ_00032266">
        <rdf:type rdf:resource="http://purl.obolibrary.org/obo/ENVO_00000004"/>
        <obo:RO_0001025 rdf:resource="http://purl.obolibrary.org/obo/GAZ_00000688"/>
        <obo:IAO_0000115>A district of South Dafur State.</obo:IAO_0000115>
        <oboInOwl:hasOBONamespace>GAZ</oboInOwl:hasOBONamespace>
        <oboInOwl:id>GAZ:00032266</oboInOwl:id>
        <rdfs:label>Al Deain District</rdfs:label>
    </owl:NamedIndividual>
    


    <!-- http://purl.obolibrary.org/obo/GAZ_00032267 -->

    <owl:NamedIndividual rdf:about="http://purl.obolibrary.org/obo/GAZ_00032267">
        <rdf:type rdf:resource="http://purl.obolibrary.org/obo/ENVO_00000004"/>
        <obo:RO_0001025 rdf:resource="http://purl.obolibrary.org/obo/GAZ_00000688"/>
        <obo:IAO_0000115>A district of South Dafur State.</obo:IAO_0000115>
        <oboInOwl:hasOBONamespace>GAZ</oboInOwl:hasOBONamespace>
        <oboInOwl:id>GAZ:00032267</oboInOwl:id>
        <rdfs:label>Tulus District</rdfs:label>
    </owl:NamedIndividual>
    


    <!-- http://purl.obolibrary.org/obo/GAZ_00032268 -->

    <owl:NamedIndividual rdf:about="http://purl.obolibrary.org/obo/GAZ_00032268">
        <rdf:type rdf:resource="http://purl.obolibrary.org/obo/ENVO_00000004"/>
        <obo:RO_0001025 rdf:resource="http://purl.obolibrary.org/obo/GAZ_00000688"/>
        <obo:IAO_0000115>A district of South Dafur State.</obo:IAO_0000115>
        <oboInOwl:hasOBONamespace>GAZ</oboInOwl:hasOBONamespace>
        <oboInOwl:id>GAZ:00032268</oboInOwl:id>
        <rdfs:label>Rehed al Birdi District</rdfs:label>
    </owl:NamedIndividual>
    


    <!-- http://purl.obolibrary.org/obo/GAZ_00032269 -->

    <owl:NamedIndividual rdf:about="http://purl.obolibrary.org/obo/GAZ_00032269">
        <rdf:type rdf:resource="http://purl.obolibrary.org/obo/ENVO_00000004"/>
        <obo:RO_0001025 rdf:resource="http://purl.obolibrary.org/obo/GAZ_00000687"/>
        <obo:IAO_0000115>A district of Sennar State.</obo:IAO_0000115>
        <oboInOwl:hasOBONamespace>GAZ</oboInOwl:hasOBONamespace>
        <oboInOwl:id>GAZ:00032269</oboInOwl:id>
        <rdfs:label>Singa District</rdfs:label>
    </owl:NamedIndividual>
    


    <!-- http://purl.obolibrary.org/obo/GAZ_00032270 -->

    <owl:NamedIndividual rdf:about="http://purl.obolibrary.org/obo/GAZ_00032270">
        <rdf:type rdf:resource="http://purl.obolibrary.org/obo/ENVO_00000004"/>
        <obo:RO_0001025 rdf:resource="http://purl.obolibrary.org/obo/GAZ_00000687"/>
        <obo:IAO_0000115>A district of Sennar State.</obo:IAO_0000115>
        <oboInOwl:hasOBONamespace>GAZ</oboInOwl:hasOBONamespace>
        <oboInOwl:id>GAZ:00032270</oboInOwl:id>
        <rdfs:label>Ad Dinder District</rdfs:label>
    </owl:NamedIndividual>
    


    <!-- http://purl.obolibrary.org/obo/GAZ_00032271 -->

    <owl:NamedIndividual rdf:about="http://purl.obolibrary.org/obo/GAZ_00032271">
        <rdf:type rdf:resource="http://purl.obolibrary.org/obo/ENVO_00000004"/>
        <obo:RO_0001025 rdf:resource="http://purl.obolibrary.org/obo/GAZ_00000687"/>
        <obo:IAO_0000115>A district of Sennar State.</obo:IAO_0000115>
        <oboInOwl:hasOBONamespace>GAZ</oboInOwl:hasOBONamespace>
        <oboInOwl:id>GAZ:00032271</oboInOwl:id>
        <rdfs:label>Sennar District</rdfs:label>
    </owl:NamedIndividual>
    


    <!-- http://purl.obolibrary.org/obo/GAZ_00032272 -->

    <owl:NamedIndividual rdf:about="http://purl.obolibrary.org/obo/GAZ_00032272">
        <rdf:type rdf:resource="http://purl.obolibrary.org/obo/ENVO_00000004"/>
        <obo:RO_0001025 rdf:resource="http://purl.obolibrary.org/obo/GAZ_00000686"/>
        <obo:IAO_0000115>A district of River Nile State.</obo:IAO_0000115>
        <oboInOwl:hasOBONamespace>GAZ</oboInOwl:hasOBONamespace>
        <oboInOwl:id>GAZ:00032272</oboInOwl:id>
        <rdfs:label>Atbara District</rdfs:label>
    </owl:NamedIndividual>
    


    <!-- http://purl.obolibrary.org/obo/GAZ_00032273 -->

    <owl:NamedIndividual rdf:about="http://purl.obolibrary.org/obo/GAZ_00032273">
        <rdf:type rdf:resource="http://purl.obolibrary.org/obo/ENVO_00000004"/>
        <obo:RO_0001025 rdf:resource="http://purl.obolibrary.org/obo/GAZ_00000686"/>
        <obo:IAO_0000115>A district of River Nile State.</obo:IAO_0000115>
        <oboInOwl:hasOBONamespace>GAZ</oboInOwl:hasOBONamespace>
        <oboInOwl:id>GAZ:00032273</oboInOwl:id>
        <rdfs:label>Shendi District</rdfs:label>
    </owl:NamedIndividual>
    


    <!-- http://purl.obolibrary.org/obo/GAZ_00032274 -->

    <owl:NamedIndividual rdf:about="http://purl.obolibrary.org/obo/GAZ_00032274">
        <rdf:type rdf:resource="http://purl.obolibrary.org/obo/ENVO_00000004"/>
        <obo:RO_0001025 rdf:resource="http://purl.obolibrary.org/obo/GAZ_00000686"/>
        <obo:IAO_0000115>A district of River Nile State.</obo:IAO_0000115>
        <oboInOwl:hasOBONamespace>GAZ</oboInOwl:hasOBONamespace>
        <oboInOwl:id>GAZ:00032274</oboInOwl:id>
        <rdfs:label>Berber District</rdfs:label>
    </owl:NamedIndividual>
    


    <!-- http://purl.obolibrary.org/obo/GAZ_00032275 -->

    <owl:NamedIndividual rdf:about="http://purl.obolibrary.org/obo/GAZ_00032275">
        <rdf:type rdf:resource="http://purl.obolibrary.org/obo/ENVO_00000004"/>
        <obo:RO_0001025 rdf:resource="http://purl.obolibrary.org/obo/GAZ_00000686"/>
        <obo:IAO_0000115>A district of River Nile State.</obo:IAO_0000115>
        <oboInOwl:hasOBONamespace>GAZ</oboInOwl:hasOBONamespace>
        <oboInOwl:id>GAZ:00032275</oboInOwl:id>
        <rdfs:label>Ad Damer District</rdfs:label>
    </owl:NamedIndividual>
    


    <!-- http://purl.obolibrary.org/obo/GAZ_00032276 -->

    <owl:NamedIndividual rdf:about="http://purl.obolibrary.org/obo/GAZ_00032276">
        <rdf:type rdf:resource="http://purl.obolibrary.org/obo/ENVO_00000004"/>
        <obo:RO_0001025 rdf:resource="http://purl.obolibrary.org/obo/GAZ_00000686"/>
        <obo:IAO_0000115>A district of River Nile State.</obo:IAO_0000115>
        <oboInOwl:hasOBONamespace>GAZ</oboInOwl:hasOBONamespace>
        <oboInOwl:id>GAZ:00032276</oboInOwl:id>
        <rdfs:label>Al Matammah District</rdfs:label>
    </owl:NamedIndividual>
    


    <!-- http://purl.obolibrary.org/obo/GAZ_00032277 -->

    <owl:NamedIndividual rdf:about="http://purl.obolibrary.org/obo/GAZ_00032277">
        <rdf:type rdf:resource="http://purl.obolibrary.org/obo/ENVO_00000004"/>
        <obo:RO_0001025 rdf:resource="http://purl.obolibrary.org/obo/GAZ_00000686"/>
        <obo:IAO_0000115>A district of River Nile State.</obo:IAO_0000115>
        <oboInOwl:hasOBONamespace>GAZ</oboInOwl:hasOBONamespace>
        <oboInOwl:id>GAZ:00032277</oboInOwl:id>
        <rdfs:label>Abu Hamad District</rdfs:label>
    </owl:NamedIndividual>
    


    <!-- http://purl.obolibrary.org/obo/GAZ_00032278 -->

    <owl:NamedIndividual rdf:about="http://purl.obolibrary.org/obo/GAZ_00032278">
        <rdf:type rdf:resource="http://purl.obolibrary.org/obo/ENVO_00000004"/>
        <obo:RO_0001025 rdf:resource="http://purl.obolibrary.org/obo/GAZ_00000685"/>
        <obo:IAO_0000115>A district of Red Sea State.</obo:IAO_0000115>
        <oboInOwl:hasOBONamespace>GAZ</oboInOwl:hasOBONamespace>
        <oboInOwl:id>GAZ:00032278</oboInOwl:id>
        <rdfs:label>Sinkat District</rdfs:label>
    </owl:NamedIndividual>
    


    <!-- http://purl.obolibrary.org/obo/GAZ_00032279 -->

    <owl:NamedIndividual rdf:about="http://purl.obolibrary.org/obo/GAZ_00032279">
        <rdf:type rdf:resource="http://purl.obolibrary.org/obo/ENVO_00000004"/>
        <obo:RO_0001025 rdf:resource="http://purl.obolibrary.org/obo/GAZ_00000685"/>
        <obo:IAO_0000115>A district of Red Sea State.</obo:IAO_0000115>
        <oboInOwl:hasOBONamespace>GAZ</oboInOwl:hasOBONamespace>
        <oboInOwl:id>GAZ:00032279</oboInOwl:id>
        <rdfs:label>Port Sudan District</rdfs:label>
    </owl:NamedIndividual>
    


    <!-- http://purl.obolibrary.org/obo/GAZ_00032280 -->

    <owl:NamedIndividual rdf:about="http://purl.obolibrary.org/obo/GAZ_00032280">
        <rdf:type rdf:resource="http://purl.obolibrary.org/obo/ENVO_00000004"/>
        <obo:RO_0001025 rdf:resource="http://purl.obolibrary.org/obo/GAZ_00000685"/>
        <obo:IAO_0000115>A district of Red Sea State.</obo:IAO_0000115>
        <oboInOwl:hasOBONamespace>GAZ</oboInOwl:hasOBONamespace>
        <oboInOwl:id>GAZ:00032280</oboInOwl:id>
        <rdfs:label>Halayeb District</rdfs:label>
    </owl:NamedIndividual>
    


    <!-- http://purl.obolibrary.org/obo/GAZ_00032281 -->

    <owl:NamedIndividual rdf:about="http://purl.obolibrary.org/obo/GAZ_00032281">
        <rdf:type rdf:resource="http://purl.obolibrary.org/obo/ENVO_00000004"/>
        <obo:RO_0001025 rdf:resource="http://purl.obolibrary.org/obo/GAZ_00000685"/>
        <obo:IAO_0000115>A district of Red Sea State.</obo:IAO_0000115>
        <oboInOwl:hasOBONamespace>GAZ</oboInOwl:hasOBONamespace>
        <oboInOwl:id>GAZ:00032281</oboInOwl:id>
        <rdfs:label>Tokar District</rdfs:label>
    </owl:NamedIndividual>
    


    <!-- http://purl.obolibrary.org/obo/GAZ_00032282 -->

    <owl:NamedIndividual rdf:about="http://purl.obolibrary.org/obo/GAZ_00032282">
        <rdf:type rdf:resource="http://purl.obolibrary.org/obo/ENVO_00000004"/>
        <obo:RO_0001025 rdf:resource="http://purl.obolibrary.org/obo/GAZ_00000684"/>
        <obo:IAO_0000115>A district of Northern State.</obo:IAO_0000115>
        <oboInOwl:hasOBONamespace>GAZ</oboInOwl:hasOBONamespace>
        <oboInOwl:id>GAZ:00032282</oboInOwl:id>
        <rdfs:label>Dongola District</rdfs:label>
    </owl:NamedIndividual>
    


    <!-- http://purl.obolibrary.org/obo/GAZ_00032283 -->

    <owl:NamedIndividual rdf:about="http://purl.obolibrary.org/obo/GAZ_00032283">
        <rdf:type rdf:resource="http://purl.obolibrary.org/obo/ENVO_00000004"/>
        <obo:RO_0001025 rdf:resource="http://purl.obolibrary.org/obo/GAZ_00000684"/>
        <obo:IAO_0000115>A district of Northern State.</obo:IAO_0000115>
        <oboInOwl:hasOBONamespace>GAZ</oboInOwl:hasOBONamespace>
        <oboInOwl:id>GAZ:00032283</oboInOwl:id>
        <rdfs:label>Merawi District</rdfs:label>
    </owl:NamedIndividual>
    


    <!-- http://purl.obolibrary.org/obo/GAZ_00032284 -->

    <owl:NamedIndividual rdf:about="http://purl.obolibrary.org/obo/GAZ_00032284">
        <rdf:type rdf:resource="http://purl.obolibrary.org/obo/ENVO_00000004"/>
        <obo:RO_0001025 rdf:resource="http://purl.obolibrary.org/obo/GAZ_00000684"/>
        <obo:IAO_0000115>A district of Northern State.</obo:IAO_0000115>
        <oboInOwl:hasOBONamespace>GAZ</oboInOwl:hasOBONamespace>
        <oboInOwl:id>GAZ:00032284</oboInOwl:id>
        <rdfs:label>Wadi Halfa District</rdfs:label>
    </owl:NamedIndividual>
    


    <!-- http://purl.obolibrary.org/obo/GAZ_00032285 -->

    <owl:NamedIndividual rdf:about="http://purl.obolibrary.org/obo/GAZ_00032285">
        <rdf:type rdf:resource="http://purl.obolibrary.org/obo/ENVO_00000004"/>
        <obo:RO_0001025 rdf:resource="http://purl.obolibrary.org/obo/GAZ_00000684"/>
        <obo:IAO_0000115>A district of Northern State.</obo:IAO_0000115>
        <oboInOwl:hasOBONamespace>GAZ</oboInOwl:hasOBONamespace>
        <oboInOwl:id>GAZ:00032285</oboInOwl:id>
        <rdfs:label>Addabah District</rdfs:label>
    </owl:NamedIndividual>
    


    <!-- http://purl.obolibrary.org/obo/GAZ_00032286 -->

    <owl:NamedIndividual rdf:about="http://purl.obolibrary.org/obo/GAZ_00032286">
        <rdf:type rdf:resource="http://purl.obolibrary.org/obo/ENVO_00000004"/>
        <obo:RO_0001025 rdf:resource="http://purl.obolibrary.org/obo/GAZ_00000683"/>
        <obo:IAO_0000115>A district of North Kurdufan State.</obo:IAO_0000115>
        <oboInOwl:hasOBONamespace>GAZ</oboInOwl:hasOBONamespace>
        <oboInOwl:id>GAZ:00032286</oboInOwl:id>
        <rdfs:label>Sheikan District</rdfs:label>
    </owl:NamedIndividual>
    


    <!-- http://purl.obolibrary.org/obo/GAZ_00032287 -->

    <owl:NamedIndividual rdf:about="http://purl.obolibrary.org/obo/GAZ_00032287">
        <rdf:type rdf:resource="http://purl.obolibrary.org/obo/ENVO_00000004"/>
        <obo:RO_0001025 rdf:resource="http://purl.obolibrary.org/obo/GAZ_00000683"/>
        <obo:IAO_0000115>A district of North Kurdufan State.</obo:IAO_0000115>
        <oboInOwl:hasOBONamespace>GAZ</oboInOwl:hasOBONamespace>
        <oboInOwl:id>GAZ:00032287</oboInOwl:id>
        <rdfs:label>Um Rawaba District</rdfs:label>
    </owl:NamedIndividual>
    


    <!-- http://purl.obolibrary.org/obo/GAZ_00032288 -->

    <owl:NamedIndividual rdf:about="http://purl.obolibrary.org/obo/GAZ_00032288">
        <rdf:type rdf:resource="http://purl.obolibrary.org/obo/ENVO_00000004"/>
        <obo:RO_0001025 rdf:resource="http://purl.obolibrary.org/obo/GAZ_00000683"/>
        <obo:IAO_0000115>A district of North Kurdufan State.</obo:IAO_0000115>
        <oboInOwl:hasOBONamespace>GAZ</oboInOwl:hasOBONamespace>
        <oboInOwl:id>GAZ:00032288</oboInOwl:id>
        <rdfs:label>Jebrat al Sheikh District</rdfs:label>
    </owl:NamedIndividual>
    


    <!-- http://purl.obolibrary.org/obo/GAZ_00032289 -->

    <owl:NamedIndividual rdf:about="http://purl.obolibrary.org/obo/GAZ_00032289">
        <rdf:type rdf:resource="http://purl.obolibrary.org/obo/ENVO_00000004"/>
        <obo:RO_0001025 rdf:resource="http://purl.obolibrary.org/obo/GAZ_00000683"/>
        <obo:IAO_0000115>A district of North Kurdufan State.</obo:IAO_0000115>
        <oboInOwl:hasOBONamespace>GAZ</oboInOwl:hasOBONamespace>
        <oboInOwl:id>GAZ:00032289</oboInOwl:id>
        <rdfs:label>Sowdari District</rdfs:label>
    </owl:NamedIndividual>
    


    <!-- http://purl.obolibrary.org/obo/GAZ_00032290 -->

    <owl:NamedIndividual rdf:about="http://purl.obolibrary.org/obo/GAZ_00032290">
        <rdf:type rdf:resource="http://purl.obolibrary.org/obo/ENVO_00000004"/>
        <obo:RO_0001025 rdf:resource="http://purl.obolibrary.org/obo/GAZ_00000683"/>
        <obo:IAO_0000115>A district of North Kurdufan State.</obo:IAO_0000115>
        <oboInOwl:hasOBONamespace>GAZ</oboInOwl:hasOBONamespace>
        <oboInOwl:id>GAZ:00032290</oboInOwl:id>
        <rdfs:label>Bara District</rdfs:label>
    </owl:NamedIndividual>
    


    <!-- http://purl.obolibrary.org/obo/GAZ_00032291 -->

    <owl:NamedIndividual rdf:about="http://purl.obolibrary.org/obo/GAZ_00032291">
        <rdf:type rdf:resource="http://purl.obolibrary.org/obo/ENVO_00000004"/>
        <obo:RO_0001025 rdf:resource="http://purl.obolibrary.org/obo/GAZ_00000682"/>
        <obo:IAO_0000115>A district of North Dafur State.</obo:IAO_0000115>
        <oboInOwl:hasOBONamespace>GAZ</oboInOwl:hasOBONamespace>
        <oboInOwl:id>GAZ:00032291</oboInOwl:id>
        <rdfs:label>Kabkabiya District</rdfs:label>
    </owl:NamedIndividual>
    


    <!-- http://purl.obolibrary.org/obo/GAZ_00032292 -->

    <owl:NamedIndividual rdf:about="http://purl.obolibrary.org/obo/GAZ_00032292">
        <rdf:type rdf:resource="http://purl.obolibrary.org/obo/ENVO_00000004"/>
        <obo:RO_0001025 rdf:resource="http://purl.obolibrary.org/obo/GAZ_00000682"/>
        <obo:IAO_0000115>A district of North Dafur State.</obo:IAO_0000115>
        <oboInOwl:hasOBONamespace>GAZ</oboInOwl:hasOBONamespace>
        <oboInOwl:id>GAZ:00032292</oboInOwl:id>
        <rdfs:label>Um Kadada District</rdfs:label>
    </owl:NamedIndividual>
    


    <!-- http://purl.obolibrary.org/obo/GAZ_00032293 -->

    <owl:NamedIndividual rdf:about="http://purl.obolibrary.org/obo/GAZ_00032293">
        <rdf:type rdf:resource="http://purl.obolibrary.org/obo/ENVO_00000004"/>
        <obo:RO_0001025 rdf:resource="http://purl.obolibrary.org/obo/GAZ_00000682"/>
        <obo:IAO_0000115>A district of North Dafur State.</obo:IAO_0000115>
        <oboInOwl:hasOBONamespace>GAZ</oboInOwl:hasOBONamespace>
        <oboInOwl:id>GAZ:00032293</oboInOwl:id>
        <rdfs:label>Kutum District</rdfs:label>
    </owl:NamedIndividual>
    


    <!-- http://purl.obolibrary.org/obo/GAZ_00032294 -->

    <owl:NamedIndividual rdf:about="http://purl.obolibrary.org/obo/GAZ_00032294">
        <rdf:type rdf:resource="http://purl.obolibrary.org/obo/ENVO_00000004"/>
        <obo:RO_0001025 rdf:resource="http://purl.obolibrary.org/obo/GAZ_00000682"/>
        <obo:IAO_0000115>A district of North Dafur State.</obo:IAO_0000115>
        <oboInOwl:hasOBONamespace>GAZ</oboInOwl:hasOBONamespace>
        <oboInOwl:id>GAZ:00032294</oboInOwl:id>
        <rdfs:label>Mellit District</rdfs:label>
    </owl:NamedIndividual>
    


    <!-- http://purl.obolibrary.org/obo/GAZ_00032295 -->

    <owl:NamedIndividual rdf:about="http://purl.obolibrary.org/obo/GAZ_00032295">
        <rdf:type rdf:resource="http://purl.obolibrary.org/obo/ENVO_00000004"/>
        <obo:RO_0001025 rdf:resource="http://purl.obolibrary.org/obo/GAZ_00000682"/>
        <obo:IAO_0000115>A district of North Dafur State.</obo:IAO_0000115>
        <oboInOwl:hasOBONamespace>GAZ</oboInOwl:hasOBONamespace>
        <oboInOwl:id>GAZ:00032295</oboInOwl:id>
        <rdfs:label>Al Fasher District</rdfs:label>
    </owl:NamedIndividual>
    


    <!-- http://purl.obolibrary.org/obo/GAZ_00032300 -->

    <owl:NamedIndividual rdf:about="http://purl.obolibrary.org/obo/GAZ_00032300">
        <rdf:type rdf:resource="http://purl.obolibrary.org/obo/ENVO_00000004"/>
        <obo:RO_0001025 rdf:resource="http://purl.obolibrary.org/obo/GAZ_00000679"/>
        <obo:IAO_0000115>A district of Khartoum State.</obo:IAO_0000115>
        <oboInOwl:hasOBONamespace>GAZ</oboInOwl:hasOBONamespace>
        <oboInOwl:id>GAZ:00032300</oboInOwl:id>
        <rdfs:label>Sharg En Nile District</rdfs:label>
    </owl:NamedIndividual>
    


    <!-- http://purl.obolibrary.org/obo/GAZ_00032301 -->

    <owl:NamedIndividual rdf:about="http://purl.obolibrary.org/obo/GAZ_00032301">
        <rdf:type rdf:resource="http://purl.obolibrary.org/obo/ENVO_00000004"/>
        <obo:RO_0001025 rdf:resource="http://purl.obolibrary.org/obo/GAZ_00000679"/>
        <obo:IAO_0000115>A district of Khartoum State.</obo:IAO_0000115>
        <oboInOwl:hasOBONamespace>GAZ</oboInOwl:hasOBONamespace>
        <oboInOwl:id>GAZ:00032301</oboInOwl:id>
        <rdfs:label>Omdurman District</rdfs:label>
    </owl:NamedIndividual>
    


    <!-- http://purl.obolibrary.org/obo/GAZ_00032302 -->

    <owl:NamedIndividual rdf:about="http://purl.obolibrary.org/obo/GAZ_00032302">
        <rdf:type rdf:resource="http://purl.obolibrary.org/obo/ENVO_00000004"/>
        <obo:RO_0001025 rdf:resource="http://purl.obolibrary.org/obo/GAZ_00000679"/>
        <obo:IAO_0000115>A district of Khartoum State.</obo:IAO_0000115>
        <oboInOwl:hasOBONamespace>GAZ</oboInOwl:hasOBONamespace>
        <oboInOwl:id>GAZ:00032302</oboInOwl:id>
        <rdfs:label>Um Badda District</rdfs:label>
    </owl:NamedIndividual>
    


    <!-- http://purl.obolibrary.org/obo/GAZ_00032304 -->

    <owl:NamedIndividual rdf:about="http://purl.obolibrary.org/obo/GAZ_00032304">
        <rdf:type rdf:resource="http://purl.obolibrary.org/obo/ENVO_00000004"/>
        <obo:RO_0001025 rdf:resource="http://purl.obolibrary.org/obo/GAZ_00000679"/>
        <obo:IAO_0000115>A district of Khartoum State.</obo:IAO_0000115>
        <oboInOwl:hasOBONamespace>GAZ</oboInOwl:hasOBONamespace>
        <oboInOwl:id>GAZ:00032304</oboInOwl:id>
        <rdfs:label>Karary District</rdfs:label>
    </owl:NamedIndividual>
    


    <!-- http://purl.obolibrary.org/obo/GAZ_00032307 -->

    <owl:NamedIndividual rdf:about="http://purl.obolibrary.org/obo/GAZ_00032307">
        <rdf:type rdf:resource="http://purl.obolibrary.org/obo/ENVO_00000004"/>
        <obo:RO_0001025 rdf:resource="http://purl.obolibrary.org/obo/GAZ_00000679"/>
        <obo:IAO_0000115>A district of Khartoum State.</obo:IAO_0000115>
        <oboInOwl:hasOBONamespace>GAZ</oboInOwl:hasOBONamespace>
        <oboInOwl:id>GAZ:00032307</oboInOwl:id>
        <rdfs:label>Khartoum District</rdfs:label>
    </owl:NamedIndividual>
    


    <!-- http://purl.obolibrary.org/obo/GAZ_00032308 -->

    <owl:NamedIndividual rdf:about="http://purl.obolibrary.org/obo/GAZ_00032308">
        <rdf:type rdf:resource="http://purl.obolibrary.org/obo/ENVO_00000004"/>
        <obo:RO_0001025 rdf:resource="http://purl.obolibrary.org/obo/GAZ_00000679"/>
        <obo:IAO_0000115>A district of Khartoum State.</obo:IAO_0000115>
        <oboInOwl:hasOBONamespace>GAZ</oboInOwl:hasOBONamespace>
        <oboInOwl:id>GAZ:00032308</oboInOwl:id>
        <rdfs:label>South Khartoum District</rdfs:label>
    </owl:NamedIndividual>
    


    <!-- http://purl.obolibrary.org/obo/GAZ_00032311 -->

    <owl:NamedIndividual rdf:about="http://purl.obolibrary.org/obo/GAZ_00032311">
        <rdf:type rdf:resource="http://purl.obolibrary.org/obo/ENVO_00000004"/>
        <obo:RO_0001025 rdf:resource="http://purl.obolibrary.org/obo/GAZ_00000679"/>
        <obo:IAO_0000115>A district of Khartoum State.</obo:IAO_0000115>
        <oboInOwl:hasOBONamespace>GAZ</oboInOwl:hasOBONamespace>
        <oboInOwl:id>GAZ:00032311</oboInOwl:id>
        <rdfs:label>Khartoum Bahri District</rdfs:label>
    </owl:NamedIndividual>
    


    <!-- http://purl.obolibrary.org/obo/GAZ_00032315 -->

    <owl:NamedIndividual rdf:about="http://purl.obolibrary.org/obo/GAZ_00032315">
        <rdf:type rdf:resource="http://purl.obolibrary.org/obo/ENVO_00000004"/>
        <obo:RO_0001025 rdf:resource="http://purl.obolibrary.org/obo/GAZ_00000678"/>
        <obo:IAO_0000115>A district of Kassala State.</obo:IAO_0000115>
        <oboInOwl:hasOBONamespace>GAZ</oboInOwl:hasOBONamespace>
        <oboInOwl:id>GAZ:00032315</oboInOwl:id>
        <rdfs:label>Hamashkorieb District</rdfs:label>
    </owl:NamedIndividual>
    


    <!-- http://purl.obolibrary.org/obo/GAZ_00032318 -->

    <owl:NamedIndividual rdf:about="http://purl.obolibrary.org/obo/GAZ_00032318">
        <rdf:type rdf:resource="http://purl.obolibrary.org/obo/ENVO_00000004"/>
        <obo:RO_0001025 rdf:resource="http://purl.obolibrary.org/obo/GAZ_00000678"/>
        <obo:IAO_0000115>A district of Kassala State.</obo:IAO_0000115>
        <oboInOwl:hasOBONamespace>GAZ</oboInOwl:hasOBONamespace>
        <oboInOwl:id>GAZ:00032318</oboInOwl:id>
        <rdfs:label>Seteet District</rdfs:label>
    </owl:NamedIndividual>
    


    <!-- http://purl.obolibrary.org/obo/GAZ_00032321 -->

    <owl:NamedIndividual rdf:about="http://purl.obolibrary.org/obo/GAZ_00032321">
        <rdf:type rdf:resource="http://purl.obolibrary.org/obo/ENVO_00000004"/>
        <obo:RO_0001025 rdf:resource="http://purl.obolibrary.org/obo/GAZ_00000678"/>
        <obo:IAO_0000115>A district of Kassala State.</obo:IAO_0000115>
        <oboInOwl:hasOBONamespace>GAZ</oboInOwl:hasOBONamespace>
        <oboInOwl:id>GAZ:00032321</oboInOwl:id>
        <rdfs:label>Nahr Atbara District</rdfs:label>
    </owl:NamedIndividual>
    


    <!-- http://purl.obolibrary.org/obo/GAZ_00032323 -->

    <owl:NamedIndividual rdf:about="http://purl.obolibrary.org/obo/GAZ_00032323">
        <rdf:type rdf:resource="http://purl.obolibrary.org/obo/ENVO_00000004"/>
        <obo:RO_0001025 rdf:resource="http://purl.obolibrary.org/obo/GAZ_00000678"/>
        <obo:IAO_0000115>A district of Kassala State.</obo:IAO_0000115>
        <oboInOwl:hasOBONamespace>GAZ</oboInOwl:hasOBONamespace>
        <oboInOwl:id>GAZ:00032323</oboInOwl:id>
        <rdfs:label>Al Gash District</rdfs:label>
    </owl:NamedIndividual>
    


    <!-- http://purl.obolibrary.org/obo/GAZ_00032324 -->

    <owl:NamedIndividual rdf:about="http://purl.obolibrary.org/obo/GAZ_00032324">
        <rdf:type rdf:resource="http://purl.obolibrary.org/obo/ENVO_00000004"/>
        <obo:RO_0001025 rdf:resource="http://purl.obolibrary.org/obo/GAZ_00000678"/>
        <obo:IAO_0000115>A district of Kassala State.</obo:IAO_0000115>
        <oboInOwl:hasOBONamespace>GAZ</oboInOwl:hasOBONamespace>
        <oboInOwl:id>GAZ:00032324</oboInOwl:id>
        <rdfs:label>Kassala District</rdfs:label>
    </owl:NamedIndividual>
    


    <!-- http://purl.obolibrary.org/obo/GAZ_00032331 -->

    <owl:NamedIndividual rdf:about="http://purl.obolibrary.org/obo/GAZ_00032331">
        <rdf:type rdf:resource="http://purl.obolibrary.org/obo/ENVO_00000004"/>
        <obo:RO_0001025 rdf:resource="http://purl.obolibrary.org/obo/GAZ_00000673"/>
        <obo:IAO_0000115>A district of Al Qadarif State.</obo:IAO_0000115>
        <oboInOwl:hasOBONamespace>GAZ</oboInOwl:hasOBONamespace>
        <oboInOwl:id>GAZ:00032331</oboInOwl:id>
        <rdfs:label>Al Gadaref District</rdfs:label>
    </owl:NamedIndividual>
    


    <!-- http://purl.obolibrary.org/obo/GAZ_00032332 -->

    <owl:NamedIndividual rdf:about="http://purl.obolibrary.org/obo/GAZ_00032332">
        <rdf:type rdf:resource="http://purl.obolibrary.org/obo/ENVO_00000004"/>
        <obo:RO_0001025 rdf:resource="http://purl.obolibrary.org/obo/GAZ_00000673"/>
        <obo:IAO_0000115>A district of Al Qadarif State.</obo:IAO_0000115>
        <oboInOwl:hasOBONamespace>GAZ</oboInOwl:hasOBONamespace>
        <oboInOwl:id>GAZ:00032332</oboInOwl:id>
        <rdfs:label>Al Faw District</rdfs:label>
    </owl:NamedIndividual>
    


    <!-- http://purl.obolibrary.org/obo/GAZ_00032333 -->

    <owl:NamedIndividual rdf:about="http://purl.obolibrary.org/obo/GAZ_00032333">
        <rdf:type rdf:resource="http://purl.obolibrary.org/obo/ENVO_00000004"/>
        <obo:RO_0001025 rdf:resource="http://purl.obolibrary.org/obo/GAZ_00000674"/>
        <obo:IAO_0000115>A district of Blue Nile State.</obo:IAO_0000115>
        <oboInOwl:hasOBONamespace>GAZ</oboInOwl:hasOBONamespace>
        <oboInOwl:id>GAZ:00032333</oboInOwl:id>
        <rdfs:label>Baw District</rdfs:label>
    </owl:NamedIndividual>
    


    <!-- http://purl.obolibrary.org/obo/GAZ_00032334 -->

    <owl:NamedIndividual rdf:about="http://purl.obolibrary.org/obo/GAZ_00032334">
        <rdf:type rdf:resource="http://purl.obolibrary.org/obo/ENVO_00000004"/>
        <obo:RO_0001025 rdf:resource="http://purl.obolibrary.org/obo/GAZ_00000674"/>
        <obo:IAO_0000115>A district of Blue Nile State.</obo:IAO_0000115>
        <oboInOwl:hasOBONamespace>GAZ</oboInOwl:hasOBONamespace>
        <oboInOwl:id>GAZ:00032334</oboInOwl:id>
        <rdfs:label>Ad Damazin District</rdfs:label>
    </owl:NamedIndividual>
    


    <!-- http://purl.obolibrary.org/obo/GAZ_00032335 -->

    <owl:NamedIndividual rdf:about="http://purl.obolibrary.org/obo/GAZ_00032335">
        <rdf:type rdf:resource="http://purl.obolibrary.org/obo/ENVO_00000004"/>
        <obo:RO_0001025 rdf:resource="http://purl.obolibrary.org/obo/GAZ_00000674"/>
        <obo:IAO_0000115>A district of Blue Nile State.</obo:IAO_0000115>
        <oboInOwl:hasOBONamespace>GAZ</oboInOwl:hasOBONamespace>
        <oboInOwl:id>GAZ:00032335</oboInOwl:id>
        <rdfs:label>Al Roseires District</rdfs:label>
    </owl:NamedIndividual>
    


    <!-- http://purl.obolibrary.org/obo/GAZ_00032336 -->

    <owl:NamedIndividual rdf:about="http://purl.obolibrary.org/obo/GAZ_00032336">
        <rdf:type rdf:resource="http://purl.obolibrary.org/obo/ENVO_00000004"/>
        <obo:RO_0001025 rdf:resource="http://purl.obolibrary.org/obo/GAZ_00000674"/>
        <obo:IAO_0000115>A district of Blue Nile State.</obo:IAO_0000115>
        <oboInOwl:hasOBONamespace>GAZ</oboInOwl:hasOBONamespace>
        <oboInOwl:id>GAZ:00032336</oboInOwl:id>
        <rdfs:label>Geissan District</rdfs:label>
    </owl:NamedIndividual>
    


    <!-- http://purl.obolibrary.org/obo/GAZ_00032337 -->

    <owl:NamedIndividual rdf:about="http://purl.obolibrary.org/obo/GAZ_00032337">
        <rdf:type rdf:resource="http://purl.obolibrary.org/obo/ENVO_00000004"/>
        <obo:RO_0001025 rdf:resource="http://purl.obolibrary.org/obo/GAZ_00000674"/>
        <obo:IAO_0000115>A district of Blue Nile State.</obo:IAO_0000115>
        <oboInOwl:hasOBONamespace>GAZ</oboInOwl:hasOBONamespace>
        <oboInOwl:id>GAZ:00032337</oboInOwl:id>
        <rdfs:label>Al Kurumik District</rdfs:label>
    </owl:NamedIndividual>
    


    <!-- http://purl.obolibrary.org/obo/GAZ_00032338 -->

    <owl:NamedIndividual rdf:about="http://purl.obolibrary.org/obo/GAZ_00032338">
        <rdf:type rdf:resource="http://purl.obolibrary.org/obo/ENVO_00000004"/>
        <obo:RO_0001025 rdf:resource="http://purl.obolibrary.org/obo/GAZ_00000673"/>
        <obo:IAO_0000115>A district of Blue Nile State.</obo:IAO_0000115>
        <oboInOwl:hasOBONamespace>GAZ</oboInOwl:hasOBONamespace>
        <oboInOwl:id>GAZ:00032338</oboInOwl:id>
        <rdfs:label>Al Rahd District</rdfs:label>
    </owl:NamedIndividual>
    


    <!-- http://purl.obolibrary.org/obo/GAZ_00032339 -->

    <owl:NamedIndividual rdf:about="http://purl.obolibrary.org/obo/GAZ_00032339">
        <rdf:type rdf:resource="http://purl.obolibrary.org/obo/ENVO_00000004"/>
        <obo:RO_0001025 rdf:resource="http://purl.obolibrary.org/obo/GAZ_00000673"/>
        <obo:IAO_0000115>A district of Al Qadarif State.</obo:IAO_0000115>
        <oboInOwl:hasOBONamespace>GAZ</oboInOwl:hasOBONamespace>
        <oboInOwl:id>GAZ:00032339</oboInOwl:id>
        <rdfs:label>Al Fushqa District</rdfs:label>
    </owl:NamedIndividual>
    


    <!-- http://purl.obolibrary.org/obo/GAZ_00032340 -->

    <owl:NamedIndividual rdf:about="http://purl.obolibrary.org/obo/GAZ_00032340">
        <rdf:type rdf:resource="http://purl.obolibrary.org/obo/ENVO_00000004"/>
        <obo:RO_0001025 rdf:resource="http://purl.obolibrary.org/obo/GAZ_00000673"/>
        <obo:IAO_0000115>A district of Al Qadarif State.</obo:IAO_0000115>
        <oboInOwl:hasOBONamespace>GAZ</oboInOwl:hasOBONamespace>
        <oboInOwl:id>GAZ:00032340</oboInOwl:id>
        <rdfs:label>Al Galabat District</rdfs:label>
    </owl:NamedIndividual>
    


    <!-- http://purl.obolibrary.org/obo/GAZ_00032341 -->

    <owl:NamedIndividual rdf:about="http://purl.obolibrary.org/obo/GAZ_00032341">
        <rdf:type rdf:resource="http://purl.obolibrary.org/obo/ENVO_00000004"/>
        <obo:RO_0001025 rdf:resource="http://purl.obolibrary.org/obo/GAZ_00000672"/>
        <obo:IAO_0000115>A district of Al Jazirah State.</obo:IAO_0000115>
        <oboInOwl:hasOBONamespace>GAZ</oboInOwl:hasOBONamespace>
        <oboInOwl:id>GAZ:00032341</oboInOwl:id>
        <rdfs:label>Al Mahagil District</rdfs:label>
    </owl:NamedIndividual>
    


    <!-- http://purl.obolibrary.org/obo/GAZ_00032342 -->

    <owl:NamedIndividual rdf:about="http://purl.obolibrary.org/obo/GAZ_00032342">
        <rdf:type rdf:resource="http://purl.obolibrary.org/obo/ENVO_00000004"/>
        <obo:RO_0001025 rdf:resource="http://purl.obolibrary.org/obo/GAZ_00000672"/>
        <obo:IAO_0000115>A district of Al Jazirah State.</obo:IAO_0000115>
        <oboInOwl:hasOBONamespace>GAZ</oboInOwl:hasOBONamespace>
        <oboInOwl:id>GAZ:00032342</oboInOwl:id>
        <rdfs:label>North al Gazera District</rdfs:label>
    </owl:NamedIndividual>
    


    <!-- http://purl.obolibrary.org/obo/GAZ_00032343 -->

    <owl:NamedIndividual rdf:about="http://purl.obolibrary.org/obo/GAZ_00032343">
        <rdf:type rdf:resource="http://purl.obolibrary.org/obo/ENVO_00000004"/>
        <obo:RO_0001025 rdf:resource="http://purl.obolibrary.org/obo/GAZ_00000672"/>
        <obo:IAO_0000115>A district of Al Jazirah State.</obo:IAO_0000115>
        <oboInOwl:hasOBONamespace>GAZ</oboInOwl:hasOBONamespace>
        <oboInOwl:id>GAZ:00032343</oboInOwl:id>
        <rdfs:label>Al Kamlin District</rdfs:label>
    </owl:NamedIndividual>
    


    <!-- http://purl.obolibrary.org/obo/GAZ_00032344 -->

    <owl:NamedIndividual rdf:about="http://purl.obolibrary.org/obo/GAZ_00032344">
        <rdf:type rdf:resource="http://purl.obolibrary.org/obo/ENVO_00000004"/>
        <obo:RO_0001025 rdf:resource="http://purl.obolibrary.org/obo/GAZ_00000672"/>
        <obo:IAO_0000115>A district of Al Jazirah State.</obo:IAO_0000115>
        <oboInOwl:hasOBONamespace>GAZ</oboInOwl:hasOBONamespace>
        <oboInOwl:id>GAZ:00032344</oboInOwl:id>
        <rdfs:label>South al Gazera District</rdfs:label>
    </owl:NamedIndividual>
    


    <!-- http://purl.obolibrary.org/obo/GAZ_00032345 -->

    <owl:NamedIndividual rdf:about="http://purl.obolibrary.org/obo/GAZ_00032345">
        <rdf:type rdf:resource="http://purl.obolibrary.org/obo/ENVO_00000004"/>
        <obo:RO_0001025 rdf:resource="http://purl.obolibrary.org/obo/GAZ_00000672"/>
        <obo:IAO_0000115>A district of Al Jazirah State.</obo:IAO_0000115>
        <oboInOwl:hasOBONamespace>GAZ</oboInOwl:hasOBONamespace>
        <oboInOwl:id>GAZ:00032345</oboInOwl:id>
        <rdfs:label>Um Al Gura District</rdfs:label>
    </owl:NamedIndividual>
    


    <!-- http://purl.obolibrary.org/obo/GAZ_00032346 -->

    <owl:NamedIndividual rdf:about="http://purl.obolibrary.org/obo/GAZ_00032346">
        <rdf:type rdf:resource="http://purl.obolibrary.org/obo/ENVO_00000004"/>
        <obo:RO_0001025 rdf:resource="http://purl.obolibrary.org/obo/GAZ_00000672"/>
        <obo:IAO_0000115>A district of Al Jazirah State.</obo:IAO_0000115>
        <oboInOwl:hasOBONamespace>GAZ</oboInOwl:hasOBONamespace>
        <oboInOwl:id>GAZ:00032346</oboInOwl:id>
        <rdfs:label>East al Gazera District</rdfs:label>
    </owl:NamedIndividual>
    


    <!-- http://purl.obolibrary.org/obo/GAZ_00032347 -->

    <owl:NamedIndividual rdf:about="http://purl.obolibrary.org/obo/GAZ_00032347">
        <rdf:type rdf:resource="http://purl.obolibrary.org/obo/ENVO_00000004"/>
        <obo:RO_0001025 rdf:resource="http://purl.obolibrary.org/obo/GAZ_00000672"/>
        <obo:IAO_0000115>A district of Al Jazirah State.</obo:IAO_0000115>
        <oboInOwl:hasOBONamespace>GAZ</oboInOwl:hasOBONamespace>
        <oboInOwl:id>GAZ:00032347</oboInOwl:id>
        <rdfs:label>Sharq al Gazera District</rdfs:label>
    </owl:NamedIndividual>
    


    <!-- http://purl.obolibrary.org/obo/GAZ_00039902 -->

    <owl:NamedIndividual rdf:about="http://purl.obolibrary.org/obo/GAZ_00039902">
        <obo:RO_0001025 rdf:resource="http://purl.obolibrary.org/obo/GAZ_00102118"/>
        <obo:IAO_0000115>A group of small islands off of the eastern coast of the Horn of Africa, in the Dact-el-Mayun section of the Bab-el-Mandeb strait.</obo:IAO_0000115>
        <oboInOwl:hasOBONamespace>GAZ</oboInOwl:hasOBONamespace>
        <oboInOwl:id>GAZ:00039902</oboInOwl:id>
        <rdfs:label>Sept Freres</rdfs:label>
    </owl:NamedIndividual>
    


    <!-- http://purl.obolibrary.org/obo/GAZ_00039909 -->

    <owl:NamedIndividual rdf:about="http://purl.obolibrary.org/obo/GAZ_00039909">
        <obo:RO_0001025 rdf:resource="http://purl.obolibrary.org/obo/GAZ_00009683"/>
        <obo:IAO_0000115>An island of the Dahlak Archipelago.</obo:IAO_0000115>
        <oboInOwl:hasOBONamespace>GAZ</oboInOwl:hasOBONamespace>
        <oboInOwl:id>GAZ:00039909</oboInOwl:id>
        <rdfs:label>Harmil Island</rdfs:label>
    </owl:NamedIndividual>
    


    <!-- http://purl.obolibrary.org/obo/GAZ_00039910 -->

    <owl:NamedIndividual rdf:about="http://purl.obolibrary.org/obo/GAZ_00039910">
        <obo:RO_0001025 rdf:resource="http://purl.obolibrary.org/obo/GAZ_00009683"/>
        <obo:IAO_0000115>An island of the Dahlak Archipelago.</obo:IAO_0000115>
        <oboInOwl:hasOBONamespace>GAZ</oboInOwl:hasOBONamespace>
        <oboInOwl:id>GAZ:00039910</oboInOwl:id>
        <rdfs:label>Nora Island</rdfs:label>
    </owl:NamedIndividual>
    


    <!-- http://purl.obolibrary.org/obo/GAZ_00039911 -->

    <owl:NamedIndividual rdf:about="http://purl.obolibrary.org/obo/GAZ_00039911">
        <obo:RO_0001025 rdf:resource="http://purl.obolibrary.org/obo/GAZ_00009683"/>
        <obo:IAO_0000115>An island of the Dahlak Archipelago.</obo:IAO_0000115>
        <oboInOwl:hasOBONamespace>GAZ</oboInOwl:hasOBONamespace>
        <oboInOwl:id>GAZ:00039911</oboInOwl:id>
        <rdfs:label>Dahlak Kebir</rdfs:label>
    </owl:NamedIndividual>
    


    <!-- http://purl.obolibrary.org/obo/GAZ_00039912 -->

    <owl:NamedIndividual rdf:about="http://purl.obolibrary.org/obo/GAZ_00039912">
        <obo:RO_0001025 rdf:resource="http://purl.obolibrary.org/obo/GAZ_00009683"/>
        <obo:IAO_0000115>An island of the Dahlak Archipelago.</obo:IAO_0000115>
        <oboInOwl:hasOBONamespace>GAZ</oboInOwl:hasOBONamespace>
        <oboInOwl:id>GAZ:00039912</oboInOwl:id>
        <rdfs:label>Nahaleg Island</rdfs:label>
    </owl:NamedIndividual>
    


    <!-- http://purl.obolibrary.org/obo/GAZ_00039913 -->

    <owl:NamedIndividual rdf:about="http://purl.obolibrary.org/obo/GAZ_00039913">
        <obo:RO_0001025 rdf:resource="http://purl.obolibrary.org/obo/GAZ_00002456"/>
        <obo:IAO_0000115>An island.</obo:IAO_0000115>
        <oboInOwl:hasOBONamespace>GAZ</oboInOwl:hasOBONamespace>
        <oboInOwl:id>GAZ:00039913</oboInOwl:id>
        <rdfs:label>Massawa Island</rdfs:label>
    </owl:NamedIndividual>
    


    <!-- http://purl.obolibrary.org/obo/GAZ_00039915 -->

    <owl:NamedIndividual rdf:about="http://purl.obolibrary.org/obo/GAZ_00039915">
        <obo:RO_0001025 rdf:resource="http://purl.obolibrary.org/obo/GAZ_00248117"/>
        <obo:IAO_0000115>An island.</obo:IAO_0000115>
        <oboInOwl:hasOBONamespace>GAZ</oboInOwl:hasOBONamespace>
        <oboInOwl:id>GAZ:00039915</oboInOwl:id>
        <rdfs:label>Halba Deset</rdfs:label>
    </owl:NamedIndividual>
    


    <!-- http://purl.obolibrary.org/obo/GAZ_00039916 -->

    <owl:NamedIndividual rdf:about="http://purl.obolibrary.org/obo/GAZ_00039916">
        <obo:RO_0001025 rdf:resource="http://purl.obolibrary.org/obo/GAZ_00002456"/>
        <obo:IAO_0000115>Islands.</obo:IAO_0000115>
        <oboInOwl:hasOBONamespace>GAZ</oboInOwl:hasOBONamespace>
        <oboInOwl:id>GAZ:00039916</oboInOwl:id>
        <rdfs:label>Howakil Islands</rdfs:label>
    </owl:NamedIndividual>
    


    <!-- http://purl.obolibrary.org/obo/GAZ_00039917 -->

    <owl:NamedIndividual rdf:about="http://purl.obolibrary.org/obo/GAZ_00039917">
        <obo:RO_0001025 rdf:resource="http://purl.obolibrary.org/obo/GAZ_00009683"/>
        <obo:IAO_0000115>An island of the Dahlak Archipelago.</obo:IAO_0000115>
        <oboInOwl:hasOBONamespace>GAZ</oboInOwl:hasOBONamespace>
        <oboInOwl:id>GAZ:00039917</oboInOwl:id>
        <rdfs:label>Isra-Tu Island</rdfs:label>
    </owl:NamedIndividual>
    


    <!-- http://purl.obolibrary.org/obo/GAZ_00039918 -->

    <owl:NamedIndividual rdf:about="http://purl.obolibrary.org/obo/GAZ_00039918">
        <obo:RO_0001025 rdf:resource="http://purl.obolibrary.org/obo/GAZ_00009683"/>
        <obo:IAO_0000115>An island of the Dahlak Archipelago.</obo:IAO_0000115>
        <oboInOwl:hasOBONamespace>GAZ</oboInOwl:hasOBONamespace>
        <oboInOwl:id>GAZ:00039918</oboInOwl:id>
        <rdfs:label>Shumma Island</rdfs:label>
    </owl:NamedIndividual>
    


    <!-- http://purl.obolibrary.org/obo/GAZ_00039919 -->

    <owl:NamedIndividual rdf:about="http://purl.obolibrary.org/obo/GAZ_00039919">
        <obo:RO_0001025 rdf:resource="http://purl.obolibrary.org/obo/GAZ_00009683"/>
        <obo:IAO_0000115>An island of the Dahlak Archipelago.</obo:IAO_0000115>
        <oboInOwl:hasOBONamespace>GAZ</oboInOwl:hasOBONamespace>
        <oboInOwl:id>GAZ:00039919</oboInOwl:id>
        <rdfs:label>Harat Island</rdfs:label>
    </owl:NamedIndividual>
    


    <!-- http://purl.obolibrary.org/obo/GAZ_00039920 -->

    <owl:NamedIndividual rdf:about="http://purl.obolibrary.org/obo/GAZ_00039920">
        <obo:RO_0001025 rdf:resource="http://purl.obolibrary.org/obo/GAZ_00009683"/>
        <obo:IAO_0000115>An island of the Dahlak Archipelago.</obo:IAO_0000115>
        <oboInOwl:hasOBONamespace>GAZ</oboInOwl:hasOBONamespace>
        <oboInOwl:id>GAZ:00039920</oboInOwl:id>
        <rdfs:label>Dissei Island</rdfs:label>
    </owl:NamedIndividual>
    


    <!-- http://purl.obolibrary.org/obo/GAZ_00039921 -->

    <owl:NamedIndividual rdf:about="http://purl.obolibrary.org/obo/GAZ_00039921">
        <obo:RO_0001025 rdf:resource="http://purl.obolibrary.org/obo/GAZ_00009683"/>
        <obo:IAO_0000115>An island of the Dahlak Archipelago.</obo:IAO_0000115>
        <oboInOwl:hasOBONamespace>GAZ</oboInOwl:hasOBONamespace>
        <oboInOwl:id>GAZ:00039921</oboInOwl:id>
        <rdfs:label>Erwa Island</rdfs:label>
    </owl:NamedIndividual>
    


    <!-- http://purl.obolibrary.org/obo/GAZ_00039922 -->

    <owl:NamedIndividual rdf:about="http://purl.obolibrary.org/obo/GAZ_00039922">
        <obo:RO_0001025 rdf:resource="http://purl.obolibrary.org/obo/GAZ_00009683"/>
        <obo:IAO_0000115>An island of the Dahlak Archipelago.</obo:IAO_0000115>
        <oboInOwl:hasOBONamespace>GAZ</oboInOwl:hasOBONamespace>
        <oboInOwl:id>GAZ:00039922</oboInOwl:id>
        <rdfs:label>Dohul Island</rdfs:label>
    </owl:NamedIndividual>
    


    <!-- http://purl.obolibrary.org/obo/GAZ_00039923 -->

    <owl:NamedIndividual rdf:about="http://purl.obolibrary.org/obo/GAZ_00039923">
        <obo:RO_0001025 rdf:resource="http://purl.obolibrary.org/obo/GAZ_00009683"/>
        <obo:IAO_0000115>An island of the Dahlak Archipelago.</obo:IAO_0000115>
        <oboInOwl:hasOBONamespace>GAZ</oboInOwl:hasOBONamespace>
        <oboInOwl:id>GAZ:00039923</oboInOwl:id>
        <rdfs:label>Dhuladhiya Island</rdfs:label>
    </owl:NamedIndividual>
    


    <!-- http://purl.obolibrary.org/obo/GAZ_00043227 -->

    <owl:NamedIndividual rdf:about="http://purl.obolibrary.org/obo/GAZ_00043227">
        <obo:IAO_0000115>An island located just to the south of Aswan.</obo:IAO_0000115>
        <oboInOwl:hasOBONamespace>GAZ</oboInOwl:hasOBONamespace>
        <oboInOwl:id>GAZ:00043227</oboInOwl:id>
        <rdfs:label>Sehel Island</rdfs:label>
    </owl:NamedIndividual>
    


    <!-- http://purl.obolibrary.org/obo/GAZ_00044902 -->

    <owl:NamedIndividual rdf:about="http://purl.obolibrary.org/obo/GAZ_00044902">
        <obo:IAO_0000115>A reservoir in Egypt and northern Sudan created as a result of the construction of the Aswan High Dam across the waters of the Nile between 1958 and 1970. The lake is some 550 km long and 35 km across at its widest point, which is near the Tropic of Cancer. It covers a total surface area of 5,250 km2 and has a storage capacity of some 157 km2 of water.</obo:IAO_0000115>
        <oboInOwl:hasOBONamespace>GAZ</oboInOwl:hasOBONamespace>
        <oboInOwl:id>GAZ:00044902</oboInOwl:id>
        <rdfs:label>Lake Nasser</rdfs:label>
    </owl:NamedIndividual>
    


    <!-- http://purl.obolibrary.org/obo/GAZ_00048570 -->

    <owl:NamedIndividual rdf:about="http://purl.obolibrary.org/obo/GAZ_00048570">
        <obo:RO_0001025 rdf:resource="http://purl.obolibrary.org/obo/GAZ_00002456"/>
        <oboInOwl:hasOBONamespace>GAZ</oboInOwl:hasOBONamespace>
        <oboInOwl:id>GAZ:00048570</oboInOwl:id>
        <rdfs:label>Gifatin Island</rdfs:label>
    </owl:NamedIndividual>
    


    <!-- http://purl.obolibrary.org/obo/GAZ_00048571 -->

    <owl:NamedIndividual rdf:about="http://purl.obolibrary.org/obo/GAZ_00048571">
        <obo:RO_0001025 rdf:resource="http://purl.obolibrary.org/obo/GAZ_00002456"/>
        <oboInOwl:hasOBONamespace>GAZ</oboInOwl:hasOBONamespace>
        <oboInOwl:id>GAZ:00048571</oboInOwl:id>
        <rdfs:label>Qeisum Island</rdfs:label>
    </owl:NamedIndividual>
    


    <!-- http://purl.obolibrary.org/obo/GAZ_00048572 -->

    <owl:NamedIndividual rdf:about="http://purl.obolibrary.org/obo/GAZ_00048572">
        <obo:RO_0001025 rdf:resource="http://purl.obolibrary.org/obo/GAZ_00002456"/>
        <obo:IAO_0000115>An island in the Red Sea.</obo:IAO_0000115>
        <oboInOwl:hasOBONamespace>GAZ</oboInOwl:hasOBONamespace>
        <oboInOwl:id>GAZ:00048572</oboInOwl:id>
        <rdfs:label>Tawila Island</rdfs:label>
    </owl:NamedIndividual>
    


    <!-- http://purl.obolibrary.org/obo/GAZ_00048573 -->

    <owl:NamedIndividual rdf:about="http://purl.obolibrary.org/obo/GAZ_00048573">
        <obo:RO_0001025 rdf:resource="http://purl.obolibrary.org/obo/GAZ_00002456"/>
        <oboInOwl:hasOBONamespace>GAZ</oboInOwl:hasOBONamespace>
        <oboInOwl:id>GAZ:00048573</oboInOwl:id>
        <rdfs:label>Gubal Island</rdfs:label>
    </owl:NamedIndividual>
    


    <!-- http://purl.obolibrary.org/obo/GAZ_00049003 -->

    <owl:NamedIndividual rdf:about="http://purl.obolibrary.org/obo/GAZ_00049003">
        <obo:RO_0001025 rdf:resource="http://purl.obolibrary.org/obo/GAZ_00002456"/>
        <obo:IAO_0000115>A large coral island group in the Red Sea, belonging to Saudi Arabia. It is located some 40 km offshore from Jizan, in the far southwestern part of the country.</obo:IAO_0000115>
        <oboInOwl:hasOBONamespace>GAZ</oboInOwl:hasOBONamespace>
        <oboInOwl:id>GAZ:00049003</oboInOwl:id>
        <rdfs:label>Farasan Islands</rdfs:label>
    </owl:NamedIndividual>
    


    <!-- http://purl.obolibrary.org/obo/GAZ_00049004 -->

    <owl:NamedIndividual rdf:about="http://purl.obolibrary.org/obo/GAZ_00049004">
        <obo:RO_0001025 rdf:resource="http://purl.obolibrary.org/obo/GAZ_00049003"/>
        <obo:IAO_0000115>One of the Farasan Islands in Saudi Arabia.</obo:IAO_0000115>
        <oboInOwl:hasOBONamespace>GAZ</oboInOwl:hasOBONamespace>
        <oboInOwl:id>GAZ:00049004</oboInOwl:id>
        <rdfs:label>Zufaf Island</rdfs:label>
    </owl:NamedIndividual>
    


    <!-- http://purl.obolibrary.org/obo/GAZ_00049005 -->

    <owl:NamedIndividual rdf:about="http://purl.obolibrary.org/obo/GAZ_00049005">
        <obo:RO_0001025 rdf:resource="http://purl.obolibrary.org/obo/GAZ_00049003"/>
        <obo:IAO_0000115>One of the Farasan Islands in Saudi Arabia.</obo:IAO_0000115>
        <oboInOwl:hasOBONamespace>GAZ</oboInOwl:hasOBONamespace>
        <oboInOwl:id>GAZ:00049005</oboInOwl:id>
        <rdfs:label>Sajid Island</rdfs:label>
    </owl:NamedIndividual>
    


    <!-- http://purl.obolibrary.org/obo/GAZ_00049006 -->

    <owl:NamedIndividual rdf:about="http://purl.obolibrary.org/obo/GAZ_00049006">
        <obo:RO_0001025 rdf:resource="http://purl.obolibrary.org/obo/GAZ_00049003"/>
        <obo:IAO_0000115>The largest island of the Farasan Islands, in the Red Sea. It is located some 50 km offshore from Jizan, the far southwestern part of Saudi Arabia.</obo:IAO_0000115>
        <oboInOwl:hasOBONamespace>GAZ</oboInOwl:hasOBONamespace>
        <oboInOwl:id>GAZ:00049006</oboInOwl:id>
        <rdfs:label>Farasan Island</rdfs:label>
    </owl:NamedIndividual>
    


    <!-- http://purl.obolibrary.org/obo/GAZ_00049021 -->

    <owl:NamedIndividual rdf:about="http://purl.obolibrary.org/obo/GAZ_00049021">
        <obo:RO_0001025 rdf:resource="http://purl.obolibrary.org/obo/GAZ_00002456"/>
        <obo:IAO_0000115>An island in the Red Sea.</obo:IAO_0000115>
        <oboInOwl:hasOBONamespace>GAZ</oboInOwl:hasOBONamespace>
        <oboInOwl:id>GAZ:00049021</oboInOwl:id>
        <rdfs:label>Jazirat Antufish</rdfs:label>
    </owl:NamedIndividual>
    


    <!-- http://purl.obolibrary.org/obo/GAZ_00051094 -->

    <owl:NamedIndividual rdf:about="http://purl.obolibrary.org/obo/GAZ_00051094">
        <obo:RO_0001025 rdf:resource="http://purl.obolibrary.org/obo/GAZ_00002456"/>
        <oboInOwl:hasOBONamespace>GAZ</oboInOwl:hasOBONamespace>
        <oboInOwl:id>GAZ:00051094</oboInOwl:id>
        <rdfs:label>Strait of Gubal</rdfs:label>
    </owl:NamedIndividual>
    


    <!-- http://purl.obolibrary.org/obo/GAZ_00051196 -->

    <owl:NamedIndividual rdf:about="http://purl.obolibrary.org/obo/GAZ_00051196">
        <obo:RO_0001025 rdf:resource="http://purl.obolibrary.org/obo/GAZ_00051197"/>
        <obo:IAO_0000115>A desert basin within the Libyan Desert of north-western Egypt. It is bounded by a steep, and in places precipitous, escarpment, along the northwestern and northern sides, which rises to heights of over 300 m, and a few km away from the escarpment edge, to over 500 m. By contrast the southern and eastern sides of the depression rise more gradually to the plateau of the Western Desert. Saline marshes/deserts, up to 30 km wide and over 150 km long, are situated under the escarpment along the northern side of the depression, and other marshes extend out into the southern central part of the basin.</obo:IAO_0000115>
        <oboInOwl:hasOBONamespace>GAZ</oboInOwl:hasOBONamespace>
        <oboInOwl:id>GAZ:00051196</oboInOwl:id>
        <rdfs:label>Qattara Depression</rdfs:label>
    </owl:NamedIndividual>
    


    <!-- http://purl.obolibrary.org/obo/GAZ_00051197 -->

    <owl:NamedIndividual rdf:about="http://purl.obolibrary.org/obo/GAZ_00051197">
        <obo:IAO_0000115>A desert that is located in the northern and eastern part of the Sahara Desert and occupies southwestern Egypt, eastern Libya and northwestern Sudan. Covering an area of approximately 1,100,000 km2 it extends approximately 1,100 km from east to west, and 1,000 km from north to south, in about the shape of a rectangle.</obo:IAO_0000115>
        <oboInOwl:hasOBONamespace>GAZ</oboInOwl:hasOBONamespace>
        <oboInOwl:id>GAZ:00051197</oboInOwl:id>
        <rdfs:label>Libyan Desert</rdfs:label>
    </owl:NamedIndividual>
    


    <!-- http://purl.obolibrary.org/obo/GAZ_00051198 -->

    <owl:NamedIndividual rdf:about="http://purl.obolibrary.org/obo/GAZ_00051198">
        <obo:IAO_0000115>A desert region in the south central Sahara. It comprises a vast plain of sand stretching from northeastern Niger into western Chad, occupying an area of over 400,000 km2). Its boundaries are conventionally said to be the Air Mountains in the west, the Ahaggar Mountains in the north, the Djado Plateau in the northeast, the Tibesti Mountains in the east and the basin of Lake Chad in the south.</obo:IAO_0000115>
        <oboInOwl:hasOBONamespace>GAZ</oboInOwl:hasOBONamespace>
        <oboInOwl:id>GAZ:00051198</oboInOwl:id>
        <rdfs:label>Erg of Tenere</rdfs:label>
    </owl:NamedIndividual>
    


    <!-- http://purl.obolibrary.org/obo/GAZ_00051199 -->

    <owl:NamedIndividual rdf:about="http://purl.obolibrary.org/obo/GAZ_00051199">
        <obo:RO_0001025 rdf:resource="http://purl.obolibrary.org/obo/GAZ_00051197"/>
        <obo:IAO_0000115>A sand sea.</obo:IAO_0000115>
        <oboInOwl:hasOBONamespace>GAZ</oboInOwl:hasOBONamespace>
        <oboInOwl:id>GAZ:00051199</oboInOwl:id>
        <rdfs:label>Rebiana Sand Sea</rdfs:label>
    </owl:NamedIndividual>
    


    <!-- http://purl.obolibrary.org/obo/GAZ_00051200 -->

    <owl:NamedIndividual rdf:about="http://purl.obolibrary.org/obo/GAZ_00051200">
        <obo:RO_0001025 rdf:resource="http://purl.obolibrary.org/obo/GAZ_00051197"/>
        <obo:IAO_0000115>A sand sea.</obo:IAO_0000115>
        <oboInOwl:hasOBONamespace>GAZ</oboInOwl:hasOBONamespace>
        <oboInOwl:id>GAZ:00051200</oboInOwl:id>
        <rdfs:label>Egyptian Sand Sea</rdfs:label>
    </owl:NamedIndividual>
    


    <!-- http://purl.obolibrary.org/obo/GAZ_00051201 -->

    <owl:NamedIndividual rdf:about="http://purl.obolibrary.org/obo/GAZ_00051201">
        <obo:RO_0001025 rdf:resource="http://purl.obolibrary.org/obo/GAZ_00051197"/>
        <obo:IAO_0000115>A sand sea.</obo:IAO_0000115>
        <oboInOwl:hasOBONamespace>GAZ</oboInOwl:hasOBONamespace>
        <oboInOwl:id>GAZ:00051201</oboInOwl:id>
        <rdfs:label>Kalansho Sand Sea</rdfs:label>
    </owl:NamedIndividual>
    


    <!-- http://purl.obolibrary.org/obo/GAZ_00051202 -->

    <owl:NamedIndividual rdf:about="http://purl.obolibrary.org/obo/GAZ_00051202">
        <obo:RO_0001025 rdf:resource="http://purl.obolibrary.org/obo/GAZ_00051198"/>
        <obo:IAO_0000115>A dune sea that stretches from Fachi, east of the Air Mountains in north central Niger, east past the town of Bilma, on to the Chadian border. It surrounds on three sides the oasis of Bilma, southernmost of a north south string of oasies of the Kaouar rise.</obo:IAO_0000115>
        <oboInOwl:hasOBONamespace>GAZ</oboInOwl:hasOBONamespace>
        <oboInOwl:id>GAZ:00051202</oboInOwl:id>
        <rdfs:label>Erg of Bilma</rdfs:label>
    </owl:NamedIndividual>
    


    <!-- http://purl.obolibrary.org/obo/GAZ_00051203 -->

    <owl:NamedIndividual rdf:about="http://purl.obolibrary.org/obo/GAZ_00051203">
        <obo:RO_0001025 rdf:resource="http://purl.obolibrary.org/obo/GAZ_00004033"/>
        <obo:IAO_0000115>A sand sea. An that is 22 km long (North-South) and 5 km wide. Its dunes reach a maximum height of 150 meters. It is located roughly 40 km south-east of Erfoud.</obo:IAO_0000115>
        <oboInOwl:hasOBONamespace>GAZ</oboInOwl:hasOBONamespace>
        <oboInOwl:id>GAZ:00051203</oboInOwl:id>
        <rdfs:label>Erg Chebbi</rdfs:label>
    </owl:NamedIndividual>
    


    <!-- http://purl.obolibrary.org/obo/GAZ_00051269 -->

    <owl:NamedIndividual rdf:about="http://purl.obolibrary.org/obo/GAZ_00051269">
        <obo:RO_0001025 rdf:resource="http://purl.obolibrary.org/obo/GAZ_00002456"/>
        <obo:IAO_0000115>A strait connecting the Red Sea to the Indian Ocean in the Gulf of Aden. The Yemeni island of Perim divides the strait into two channels.</obo:IAO_0000115>
        <oboInOwl:hasOBONamespace>GAZ</oboInOwl:hasOBONamespace>
        <oboInOwl:id>GAZ:00051269</oboInOwl:id>
        <rdfs:label>Bab-el-Mandeb</rdfs:label>
    </owl:NamedIndividual>
    


    <!-- http://purl.obolibrary.org/obo/GAZ_00052553 -->

    <owl:NamedIndividual rdf:about="http://purl.obolibrary.org/obo/GAZ_00052553">
        <obo:IAO_0000115>A river that rises in the central highlands of Ethiopia near Mount Qachen, from where it flows west, north, then west again, forming the westernmost border of Ethiopia and Eritrea. The river continues into northeastern Sudan, where at 14deg10minN, 36degE, the Tekeze joins the Atbarah River, the lower course of which is a tributary of the Nile. The Tekeze is perhaps the true upper course of the Atbarah, as the former follows the longer course prior to the confluence of the two rivers. The names of its main tributaries in Ethiopia from its source are: on the right bank Tahali, Meri, Sellare, Sullo, Arekwa, Gheoa, Wari, Firafira, Tocoro and Gumalo Rivers; on the left bank Nili, Balagas, Saha, Bembea, Ataba, Zarima, and Kwalema Rivers.</obo:IAO_0000115>
        <oboInOwl:hasOBONamespace>GAZ</oboInOwl:hasOBONamespace>
        <oboInOwl:id>GAZ:00052553</oboInOwl:id>
        <rdfs:label>Tekeze River</rdfs:label>
    </owl:NamedIndividual>
    


    <!-- http://purl.obolibrary.org/obo/GAZ_00053489 -->

    <owl:NamedIndividual rdf:about="http://purl.obolibrary.org/obo/GAZ_00053489">
        <obo:RO_0001025 rdf:resource="http://purl.obolibrary.org/obo/GAZ_00103898"/>
        <obo:IAO_0000115>A volcanic field covers a broad area of about 1050 km2 in the Tuareg shield in the southern Air region of Niger. Activity began with the eruption of about 30 trachytic and phonolitic volcanoes through Precambrian basement rocks. This was followed by the formation of about 130 basaltic cones that typically produced a valley filling lava flow. A series of NW-SE-trending faults control volcano locations.</obo:IAO_0000115>
        <oboInOwl:hasOBONamespace>GAZ</oboInOwl:hasOBONamespace>
        <oboInOwl:id>GAZ:00053489</oboInOwl:id>
        <rdfs:label>Todra Volcanic Field</rdfs:label>
    </owl:NamedIndividual>
    


    <!-- http://purl.obolibrary.org/obo/GAZ_00053496 -->

    <owl:NamedIndividual rdf:about="http://purl.obolibrary.org/obo/GAZ_00053496">
        <obo:IAO_0000115>A volcanic field that lies in the Sahara desert of south-central Libya, south of the Haruj volcanic field. A 4 km wide, 100-m-deep caldera contains a post-caldera scoria cone, Wau-en-Namus. An apron of dark basaltic tephra extends 10-20 km around the caldera in stark contrast to the light-colored desert sand prominent in satellite views. Three small saline lakes of variable color contribute to the name of the volcano.</obo:IAO_0000115>
        <oboInOwl:hasOBONamespace>GAZ</oboInOwl:hasOBONamespace>
        <oboInOwl:id>GAZ:00053496</oboInOwl:id>
        <rdfs:label>Wau-en-Namus Volcanic Field</rdfs:label>
    </owl:NamedIndividual>
    


    <!-- http://purl.obolibrary.org/obo/GAZ_00053504 -->

    <owl:NamedIndividual rdf:about="http://purl.obolibrary.org/obo/GAZ_00053504">
        <obo:RO_0001025 rdf:resource="http://purl.obolibrary.org/obo/GAZ_00053506"/>
        <obo:IAO_0000115>A volcanic field, located in the Darfur province of western Sudan. The Jebel Marra volcanic field covers a broad area of the Marra Mountains and contains early basaltic lava flows overlain by thick sequences of pyroclastic-flow deposits. The northern part of the volcanic field displays trachytic lava plugs and spines forming residual inselbergs and young basaltic scoria cones and lava flows.</obo:IAO_0000115>
        <oboInOwl:hasOBONamespace>GAZ</oboInOwl:hasOBONamespace>
        <oboInOwl:id>GAZ:00053504</oboInOwl:id>
        <rdfs:label>Jebel Marra Volcanic Field</rdfs:label>
    </owl:NamedIndividual>
    


    <!-- http://purl.obolibrary.org/obo/GAZ_00053505 -->

    <owl:NamedIndividual rdf:about="http://purl.obolibrary.org/obo/GAZ_00053505">
        <obo:RO_0001025 rdf:resource="http://purl.obolibrary.org/obo/GAZ_00053504"/>
        <obo:IAO_0000115>A 5 km wide, steep-walled caldera, located at the southern end of the volcanic field, was formed about 3500 years ago at the time of the eruption of voluminous airfall pumice and pyroclastic flows that traveled more than 30 km from the volcano.</obo:IAO_0000115>
        <oboInOwl:hasOBONamespace>GAZ</oboInOwl:hasOBONamespace>
        <oboInOwl:id>GAZ:00053505</oboInOwl:id>
        <rdfs:label>Deriba Caldera</rdfs:label>
    </owl:NamedIndividual>
    


    <!-- http://purl.obolibrary.org/obo/GAZ_00053506 -->

    <owl:NamedIndividual rdf:about="http://purl.obolibrary.org/obo/GAZ_00053506">
        <rdf:type rdf:resource="http://purl.obolibrary.org/obo/ENVO_00000106"/>
        <obo:RO_0001025 rdf:resource="http://purl.obolibrary.org/obo/GAZ_00004036"/>
        <obo:IAO_0000115>A range of volcanic peaks created by a massif that rises up to 3,000 m. It is located in the center of the Darfur region of Sudan, specifically within Dar Zagahawa and neighboring areas. The highest point is Deriba Crater.</obo:IAO_0000115>
        <oboInOwl:hasOBONamespace>GAZ</oboInOwl:hasOBONamespace>
        <oboInOwl:id>GAZ:00053506</oboInOwl:id>
        <rdfs:label>Marrah Mountains</rdfs:label>
    </owl:NamedIndividual>
    


    <!-- http://purl.obolibrary.org/obo/GAZ_00053507 -->

    <owl:NamedIndividual rdf:about="http://purl.obolibrary.org/obo/GAZ_00053507">
        <obo:RO_0001025 rdf:resource="http://purl.obolibrary.org/obo/GAZ_00004036"/>
        <obo:IAO_0000115>A basaltic volcanic field (scoria cones) in the northern Dafur area of western Sudan, is located SW of the larger Meidob volcanic field.</obo:IAO_0000115>
        <oboInOwl:hasOBONamespace>GAZ</oboInOwl:hasOBONamespace>
        <oboInOwl:id>GAZ:00053507</oboInOwl:id>
        <rdfs:label>Kutum Volcanic Field</rdfs:label>
    </owl:NamedIndividual>
    


    <!-- http://purl.obolibrary.org/obo/GAZ_00053508 -->

    <owl:NamedIndividual rdf:about="http://purl.obolibrary.org/obo/GAZ_00053508">
        <obo:RO_0001025 rdf:resource="http://purl.obolibrary.org/obo/GAZ_00004036"/>
        <obo:IAO_0000115>A volcanic field in western Sudan, at the NE end of the Dafur volcanic province, covers an area of 5000 km2 with nearly 700 Pliocene-to-Holocene vents. The volcanic field was constructed over an uplifted Precambrian igneous and metamorphic basement and is elongated in an E-W direction. Basaltic scoria cones and associated lava flows dominate, but trachytic-phonolitic lava domes, tuff rings, and maars are among the youngest volcanic products. Basaltic scoria cones are scattered throughout the field; their lavas have produced a broad lava plateau. The central part of the field consists of younger phonolitic lava flows, trachytic pumice-fall deposits, ignimbrites, and maars.</obo:IAO_0000115>
        <oboInOwl:hasOBONamespace>GAZ</oboInOwl:hasOBONamespace>
        <oboInOwl:id>GAZ:00053508</oboInOwl:id>
        <rdfs:label>Meidob Volcanic Field</rdfs:label>
    </owl:NamedIndividual>
    


    <!-- http://purl.obolibrary.org/obo/GAZ_00053509 -->

    <owl:NamedIndividual rdf:about="http://purl.obolibrary.org/obo/GAZ_00053509">
        <obo:RO_0001025 rdf:resource="http://purl.obolibrary.org/obo/GAZ_00057756"/>
        <obo:IAO_0000115>A volcanic field is located in the Bayuda Desert of NE Sudan, south of the major Abu Hamed bend of the Nile River about 300 km north of capital city of Khartoum. More than 90 eruptive centers along a WNW-ESE line were constructed over Precambrian and Paleozoic granitic rocks near the center of the Bayuda Desert. Most vents of the Bayuda field are cinder cones that produced lava flows which breached the cones. About 10% of vents in the field are explosion craters, the largest of which, named Hosh ed Dalam, is 1.3 km wide and up to 500 m deep.</obo:IAO_0000115>
        <oboInOwl:hasOBONamespace>GAZ</oboInOwl:hasOBONamespace>
        <oboInOwl:id>GAZ:00053509</oboInOwl:id>
        <rdfs:label>Bayuda Volcanic Field</rdfs:label>
    </owl:NamedIndividual>
    


    <!-- http://purl.obolibrary.org/obo/GAZ_00053510 -->

    <owl:NamedIndividual rdf:about="http://purl.obolibrary.org/obo/GAZ_00053510">
        <obo:RO_0001025 rdf:resource="http://purl.obolibrary.org/obo/GAZ_00053509"/>
        <obo:IAO_0000115>A volanic crater.</obo:IAO_0000115>
        <oboInOwl:hasOBONamespace>GAZ</oboInOwl:hasOBONamespace>
        <oboInOwl:id>GAZ:00053510</oboInOwl:id>
        <rdfs:label>Hosh ed Dalam</rdfs:label>
    </owl:NamedIndividual>
    


    <!-- http://purl.obolibrary.org/obo/GAZ_00053511 -->

    <owl:NamedIndividual rdf:about="http://purl.obolibrary.org/obo/GAZ_00053511">
        <obo:RO_0001025 rdf:resource="http://purl.obolibrary.org/obo/GAZ_00057756"/>
        <obo:IAO_0000115>A volcanic field (shield volcano) located in the Bayuda desert of NE Sudan, immediately west of the Nile River, NE of the capital city of Khartoum. Jebel Umm Arafieb consists of a low-angle shield volcano of basanitic-to-trachybasaltic composition formed of several overlapping aa lava flows erupted from a vent now capped by a spatter cone.</obo:IAO_0000115>
        <oboInOwl:hasOBONamespace>GAZ</oboInOwl:hasOBONamespace>
        <oboInOwl:id>GAZ:00053511</oboInOwl:id>
        <rdfs:label>Jebel Umm Arafieb Volcanic Field</rdfs:label>
    </owl:NamedIndividual>
    


    <!-- http://purl.obolibrary.org/obo/GAZ_00053592 -->

    <owl:NamedIndividual rdf:about="http://purl.obolibrary.org/obo/GAZ_00053592">
        <obo:RO_0001025 rdf:resource="http://purl.obolibrary.org/obo/GAZ_00002456"/>
        <obo:IAO_0000115>A stratovolcano rises from a 1200 m depth in the south-central Red Sea, forming an oval-shaped island about 3 km long. Located northwest of the constricted Bab al-Mandab passage at the mouth of the Red Sea, about half way between Yemen and Eritrea.</obo:IAO_0000115>
        <oboInOwl:hasOBONamespace>GAZ</oboInOwl:hasOBONamespace>
        <oboInOwl:id>GAZ:00053592</oboInOwl:id>
        <rdfs:label>Jabal al-Tair Island</rdfs:label>
    </owl:NamedIndividual>
    


    <!-- http://purl.obolibrary.org/obo/GAZ_00053593 -->

    <owl:NamedIndividual rdf:about="http://purl.obolibrary.org/obo/GAZ_00053593">
        <obo:RO_0001025 rdf:resource="http://purl.obolibrary.org/obo/GAZ_00053592"/>
        <obo:IAO_0000115>A volcanic vent.</obo:IAO_0000115>
        <oboInOwl:hasOBONamespace>GAZ</oboInOwl:hasOBONamespace>
        <oboInOwl:id>GAZ:00053593</oboInOwl:id>
        <rdfs:label>Jebel Duchan</rdfs:label>
    </owl:NamedIndividual>
    


    <!-- http://purl.obolibrary.org/obo/GAZ_00053594 -->

    <owl:NamedIndividual rdf:about="http://purl.obolibrary.org/obo/GAZ_00053594">
        <obo:RO_0001025 rdf:resource="http://purl.obolibrary.org/obo/GAZ_00002456"/>
        <obo:IAO_0000115>The largest of a group of 10 small islands and submerged shoals that rise from a shallow platform in the Red Sea rift.</obo:IAO_0000115>
        <oboInOwl:hasOBONamespace>GAZ</oboInOwl:hasOBONamespace>
        <oboInOwl:id>GAZ:00053594</oboInOwl:id>
        <rdfs:label>Jebel Zubair</rdfs:label>
    </owl:NamedIndividual>
    


    <!-- http://purl.obolibrary.org/obo/GAZ_00053595 -->

    <owl:NamedIndividual rdf:about="http://purl.obolibrary.org/obo/GAZ_00053595">
        <obo:RO_0001025 rdf:resource="http://purl.obolibrary.org/obo/GAZ_00005876"/>
        <obo:IAO_0000115>The largest of the Hanish Islands, which belong to Yemen.</obo:IAO_0000115>
        <oboInOwl:hasOBONamespace>GAZ</oboInOwl:hasOBONamespace>
        <oboInOwl:id>GAZ:00053595</oboInOwl:id>
        <rdfs:label>Great Hanish Island</rdfs:label>
    </owl:NamedIndividual>
    


    <!-- http://purl.obolibrary.org/obo/GAZ_00053596 -->

    <owl:NamedIndividual rdf:about="http://purl.obolibrary.org/obo/GAZ_00053596">
        <obo:RO_0001025 rdf:resource="http://purl.obolibrary.org/obo/GAZ_00005876"/>
        <oboInOwl:hasOBONamespace>GAZ</oboInOwl:hasOBONamespace>
        <oboInOwl:id>GAZ:00053596</oboInOwl:id>
        <rdfs:label>Little Hanish Island</rdfs:label>
    </owl:NamedIndividual>
    


    <!-- http://purl.obolibrary.org/obo/GAZ_00053597 -->

    <owl:NamedIndividual rdf:about="http://purl.obolibrary.org/obo/GAZ_00053597">
        <obo:RO_0001025 rdf:resource="http://purl.obolibrary.org/obo/GAZ_00002456"/>
        <oboInOwl:hasOBONamespace>GAZ</oboInOwl:hasOBONamespace>
        <oboInOwl:id>GAZ:00053597</oboInOwl:id>
        <rdfs:label>Zukur-Hanish island group</rdfs:label>
    </owl:NamedIndividual>
    


    <!-- http://purl.obolibrary.org/obo/GAZ_00057756 -->

    <owl:NamedIndividual rdf:about="http://purl.obolibrary.org/obo/GAZ_00057756">
        <obo:RO_0001025 rdf:resource="http://purl.obolibrary.org/obo/GAZ_00233441"/>
        <obo:IAO_0000115>A desert located north of Khartoum, Sudan, west of Kadabas, and north of the Nubian Desert, together making up part of the Sahara&apos;s eastern flank.</obo:IAO_0000115>
        <oboInOwl:hasOBONamespace>GAZ</oboInOwl:hasOBONamespace>
        <oboInOwl:id>GAZ:00057756</oboInOwl:id>
        <rdfs:label>Bayuda Desert</rdfs:label>
    </owl:NamedIndividual>
    


    <!-- http://purl.obolibrary.org/obo/GAZ_00057757 -->

    <owl:NamedIndividual rdf:about="http://purl.obolibrary.org/obo/GAZ_00057757">
        <obo:RO_0001025 rdf:resource="http://purl.obolibrary.org/obo/GAZ_00233441"/>
        <obo:IAO_0000115>The eastern region of the Sahara Desert, it spans 50, 000 km2 of northeastern Sudan between the Nile and the Red Sea.</obo:IAO_0000115>
        <oboInOwl:hasOBONamespace>GAZ</oboInOwl:hasOBONamespace>
        <oboInOwl:id>GAZ:00057757</oboInOwl:id>
        <rdfs:label>Nubian Desert</rdfs:label>
    </owl:NamedIndividual>
    


    <!-- http://purl.obolibrary.org/obo/GAZ_00057759 -->

    <owl:NamedIndividual rdf:about="http://purl.obolibrary.org/obo/GAZ_00057759">
        <obo:IAO_0000115>A desert east of the river Nile, between the Nile and the Red Sea. It extends from Egypt in the north to Eritrea in the south, and also comprises parts of Sudan and Ethiopia.</obo:IAO_0000115>
        <oboInOwl:hasOBONamespace>GAZ</oboInOwl:hasOBONamespace>
        <oboInOwl:id>GAZ:00057759</oboInOwl:id>
        <rdfs:label>Eastern Desert</rdfs:label>
    </owl:NamedIndividual>
    


    <!-- http://purl.obolibrary.org/obo/GAZ_00058791 -->

    <owl:NamedIndividual rdf:about="http://purl.obolibrary.org/obo/GAZ_00058791">
        <obo:IAO_0000115>A polymictic shallow lake complex of Uganda, about 1,720 km2 in area and at an elevation of 914 m. The Victoria Nile flows through the lake on its way from Lake Victoria to Lake Albert. The main inflow from Lake Victoria is regulated by the Nalubaale Power Station in Jinja. Another source of water is the Mount Elgon region on the border between Uganda and Kenya.</obo:IAO_0000115>
        <oboInOwl:hasOBONamespace>GAZ</oboInOwl:hasOBONamespace>
        <oboInOwl:id>GAZ:00058791</oboInOwl:id>
        <rdfs:label>Lake Kyoga</rdfs:label>
    </owl:NamedIndividual>
    


    <!-- http://purl.obolibrary.org/obo/GAZ_00058849 -->

    <owl:NamedIndividual rdf:about="http://purl.obolibrary.org/obo/GAZ_00058849">
        <obo:RO_0001025 rdf:resource="http://purl.obolibrary.org/obo/GAZ_00051197"/>
        <obo:IAO_0000115>Recently formed endorheic lakes in the Sahara Desert of Egypt. Caused by water from Lake Nasser running through the Sadat Canal.</obo:IAO_0000115>
        <oboInOwl:hasOBONamespace>GAZ</oboInOwl:hasOBONamespace>
        <oboInOwl:id>GAZ:00058849</oboInOwl:id>
        <rdfs:label>Toshka Lakes</rdfs:label>
    </owl:NamedIndividual>
    


    <!-- http://purl.obolibrary.org/obo/GAZ_00058872 -->

    <owl:NamedIndividual rdf:about="http://purl.obolibrary.org/obo/GAZ_00058872">
        <obo:IAO_0000115>The two dams at the first cataract on the Nile in Egypt.</obo:IAO_0000115>
        <oboInOwl:hasOBONamespace>GAZ</oboInOwl:hasOBONamespace>
        <oboInOwl:id>GAZ:00058872</oboInOwl:id>
        <rdfs:label>Aswan Dams</rdfs:label>
    </owl:NamedIndividual>
    


    <!-- http://purl.obolibrary.org/obo/GAZ_00058873 -->

    <owl:NamedIndividual rdf:about="http://purl.obolibrary.org/obo/GAZ_00058873">
        <obo:RO_0001025 rdf:resource="http://purl.obolibrary.org/obo/GAZ_00058872"/>
        <obo:IAO_0000115>The newer of the Aswan Dams, completed in 1968. It is located 7 km south of Aswan City.</obo:IAO_0000115>
        <oboInOwl:hasOBONamespace>GAZ</oboInOwl:hasOBONamespace>
        <oboInOwl:id>GAZ:00058873</oboInOwl:id>
        <rdfs:label>Aswan High Dam</rdfs:label>
    </owl:NamedIndividual>
    


    <!-- http://purl.obolibrary.org/obo/GAZ_00058874 -->

    <owl:NamedIndividual rdf:about="http://purl.obolibrary.org/obo/GAZ_00058874">
        <obo:RO_0001025 rdf:resource="http://purl.obolibrary.org/obo/GAZ_00058872"/>
        <obo:IAO_0000115>The first of the Aswan Dams on the Nile, finished in 1902.</obo:IAO_0000115>
        <oboInOwl:hasOBONamespace>GAZ</oboInOwl:hasOBONamespace>
        <oboInOwl:id>GAZ:00058874</oboInOwl:id>
        <rdfs:label>Aswan Low Dam</rdfs:label>
    </owl:NamedIndividual>
    


    <!-- http://purl.obolibrary.org/obo/GAZ_00058877 -->

    <owl:NamedIndividual rdf:about="http://purl.obolibrary.org/obo/GAZ_00058877">
        <obo:RO_0001025 rdf:resource="http://purl.obolibrary.org/obo/GAZ_00009949"/>
        <obo:IAO_0000115>A dam that was completed in 1862. Its purpose was to improve irrigation in the Nile Delta area of Egypt.</obo:IAO_0000115>
        <oboInOwl:hasOBONamespace>GAZ</oboInOwl:hasOBONamespace>
        <oboInOwl:id>GAZ:00058877</oboInOwl:id>
        <rdfs:label>Delta Barrage</rdfs:label>
    </owl:NamedIndividual>
    


    <!-- http://purl.obolibrary.org/obo/GAZ_00058878 -->

    <owl:NamedIndividual rdf:about="http://purl.obolibrary.org/obo/GAZ_00058878">
        <rdf:type rdf:resource="http://purl.obolibrary.org/obo/ENVO_00000074"/>
        <obo:IAO_0000115>A barrage on the River Nile in Egypt.</obo:IAO_0000115>
        <oboInOwl:hasOBONamespace>GAZ</oboInOwl:hasOBONamespace>
        <oboInOwl:id>GAZ:00058878</oboInOwl:id>
        <rdfs:label>Esna Barrage</rdfs:label>
    </owl:NamedIndividual>
    


    <!-- http://purl.obolibrary.org/obo/GAZ_00058879 -->

    <owl:NamedIndividual rdf:about="http://purl.obolibrary.org/obo/GAZ_00058879">
        <rdf:type rdf:resource="http://purl.obolibrary.org/obo/ENVO_00000074"/>
        <obo:IAO_0000115>A barrage on the River Nile in Egypt.</obo:IAO_0000115>
        <oboInOwl:hasOBONamespace>GAZ</oboInOwl:hasOBONamespace>
        <oboInOwl:id>GAZ:00058879</oboInOwl:id>
        <rdfs:label>Nag Hammadi Barrage</rdfs:label>
    </owl:NamedIndividual>
    


    <!-- http://purl.obolibrary.org/obo/GAZ_00058880 -->

    <owl:NamedIndividual rdf:about="http://purl.obolibrary.org/obo/GAZ_00058880">
        <rdf:type rdf:resource="http://purl.obolibrary.org/obo/ENVO_00000074"/>
        <obo:IAO_0000115>A barrage on the River Nile in Egypt.</obo:IAO_0000115>
        <oboInOwl:hasOBONamespace>GAZ</oboInOwl:hasOBONamespace>
        <oboInOwl:id>GAZ:00058880</oboInOwl:id>
        <rdfs:label>Assuit Barrage</rdfs:label>
    </owl:NamedIndividual>
    


    <!-- http://purl.obolibrary.org/obo/GAZ_00058881 -->

    <owl:NamedIndividual rdf:about="http://purl.obolibrary.org/obo/GAZ_00058881">
        <obo:IAO_0000115>A dam on the Rosetta Canal.</obo:IAO_0000115>
        <oboInOwl:hasOBONamespace>GAZ</oboInOwl:hasOBONamespace>
        <oboInOwl:id>GAZ:00058881</oboInOwl:id>
        <rdfs:label>Edfina Barrage</rdfs:label>
    </owl:NamedIndividual>
    


    <!-- http://purl.obolibrary.org/obo/GAZ_00058882 -->

    <owl:NamedIndividual rdf:about="http://purl.obolibrary.org/obo/GAZ_00058882">
        <obo:IAO_0000115>A dam on the Damietta Canal.</obo:IAO_0000115>
        <oboInOwl:hasOBONamespace>GAZ</oboInOwl:hasOBONamespace>
        <oboInOwl:id>GAZ:00058882</oboInOwl:id>
        <rdfs:label>Faraskour Barrage</rdfs:label>
    </owl:NamedIndividual>
    


    <!-- http://purl.obolibrary.org/obo/GAZ_00058883 -->

    <owl:NamedIndividual rdf:about="http://purl.obolibrary.org/obo/GAZ_00058883">
        <obo:IAO_0000115>A dam on the Damietta Canal.</obo:IAO_0000115>
        <oboInOwl:hasOBONamespace>GAZ</oboInOwl:hasOBONamespace>
        <oboInOwl:id>GAZ:00058883</oboInOwl:id>
        <rdfs:label>Zitta Barrage</rdfs:label>
    </owl:NamedIndividual>
    


    <!-- http://purl.obolibrary.org/obo/GAZ_00058884 -->

    <owl:NamedIndividual rdf:about="http://purl.obolibrary.org/obo/GAZ_00058884"/>
    


    <!-- http://purl.obolibrary.org/obo/GAZ_00058886 -->

    <owl:NamedIndividual rdf:about="http://purl.obolibrary.org/obo/GAZ_00058886"/>
    


    <!-- http://purl.obolibrary.org/obo/GAZ_00058890 -->

    <owl:NamedIndividual rdf:about="http://purl.obolibrary.org/obo/GAZ_00058890"/>
    


    <!-- http://purl.obolibrary.org/obo/GAZ_00058891 -->

    <owl:NamedIndividual rdf:about="http://purl.obolibrary.org/obo/GAZ_00058891">
        <obo:RO_0001025 rdf:resource="http://purl.obolibrary.org/obo/GAZ_00058886"/>
        <obo:IAO_0000115>An island in the River Nile in Egypt near the Fourth Cataract in Dar al-Manasir.</obo:IAO_0000115>
        <oboInOwl:hasOBONamespace>GAZ</oboInOwl:hasOBONamespace>
        <oboInOwl:id>GAZ:00058891</oboInOwl:id>
        <rdfs:label>Island of Muqrat</rdfs:label>
    </owl:NamedIndividual>
    


    <!-- http://purl.obolibrary.org/obo/GAZ_00058892 -->

    <owl:NamedIndividual rdf:about="http://purl.obolibrary.org/obo/GAZ_00058892">
        <obo:IAO_0000115>A dam under construction on the River Nile in Sudan, about 350 km north of the capital Khartoum.</obo:IAO_0000115>
        <oboInOwl:hasOBONamespace>GAZ</oboInOwl:hasOBONamespace>
        <oboInOwl:id>GAZ:00058892</oboInOwl:id>
        <rdfs:label>Merowe High Dam</rdfs:label>
    </owl:NamedIndividual>
    


    <!-- http://purl.obolibrary.org/obo/GAZ_00066409 -->

    <owl:NamedIndividual rdf:about="http://purl.obolibrary.org/obo/GAZ_00066409">
        <obo:RO_0001025 rdf:resource="http://purl.obolibrary.org/obo/GAZ_00248009"/>
        <obo:IAO_0000115>An oasis in Egypt, located between the Qattara Depression and the Egyptian Sand Sea in the Libyan Desert, nearly 50 km east of the Libyan border, and 560 km from Cairo.</obo:IAO_0000115>
        <oboInOwl:hasOBONamespace>GAZ</oboInOwl:hasOBONamespace>
        <oboInOwl:id>GAZ:00066409</oboInOwl:id>
        <rdfs:label>Siwa Oasis</rdfs:label>
    </owl:NamedIndividual>
    


    <!-- http://purl.obolibrary.org/obo/GAZ_00066410 -->

    <owl:NamedIndividual rdf:about="http://purl.obolibrary.org/obo/GAZ_00066410">
        <obo:RO_0001025 rdf:resource="http://purl.obolibrary.org/obo/GAZ_00051197"/>
        <obo:IAO_0000115>A desert located 45 km north of Farafra. The desert has a white, cream color and has massive chalk rock formations that have been created as a result of occasional sandstorms in the area.</obo:IAO_0000115>
        <oboInOwl:hasOBONamespace>GAZ</oboInOwl:hasOBONamespace>
        <oboInOwl:id>GAZ:00066410</oboInOwl:id>
        <rdfs:label>Sahara el Beyda</rdfs:label>
    </owl:NamedIndividual>
    


    <!-- http://purl.obolibrary.org/obo/GAZ_00066428 -->

    <owl:NamedIndividual rdf:about="http://purl.obolibrary.org/obo/GAZ_00066428">
        <obo:RO_0001025 rdf:resource="http://purl.obolibrary.org/obo/GAZ_00051197"/>
        <obo:IAO_0000115>An oasis with a large lake located in the municipality Sabha in the Libyan Sahara. The lake is saline.</obo:IAO_0000115>
        <oboInOwl:hasOBONamespace>GAZ</oboInOwl:hasOBONamespace>
        <oboInOwl:id>GAZ:00066428</oboInOwl:id>
        <rdfs:label>Gaberoun Oasis</rdfs:label>
    </owl:NamedIndividual>
    


    <!-- http://purl.obolibrary.org/obo/GAZ_00066429 -->

    <owl:NamedIndividual rdf:about="http://purl.obolibrary.org/obo/GAZ_00066429">
        <obo:RO_0001025 rdf:resource="http://purl.obolibrary.org/obo/GAZ_00051197"/>
        <obo:IAO_0000115>An erg.</obo:IAO_0000115>
        <oboInOwl:hasOBONamespace>GAZ</oboInOwl:hasOBONamespace>
        <oboInOwl:id>GAZ:00066429</oboInOwl:id>
        <rdfs:label>Ramlat al Dauada</rdfs:label>
    </owl:NamedIndividual>
    


    <!-- http://purl.obolibrary.org/obo/GAZ_00066430 -->

    <owl:NamedIndividual rdf:about="http://purl.obolibrary.org/obo/GAZ_00066430">
        <obo:RO_0001025 rdf:resource="http://purl.obolibrary.org/obo/GAZ_00066429"/>
        <obo:IAO_0000115>A lake in the Ramlat al Dauada erg.</obo:IAO_0000115>
        <oboInOwl:hasOBONamespace>GAZ</oboInOwl:hasOBONamespace>
        <oboInOwl:id>GAZ:00066430</oboInOwl:id>
        <rdfs:label>Mafo Lake</rdfs:label>
    </owl:NamedIndividual>
    


    <!-- http://purl.obolibrary.org/obo/GAZ_00066431 -->

    <owl:NamedIndividual rdf:about="http://purl.obolibrary.org/obo/GAZ_00066431">
        <obo:RO_0001025 rdf:resource="http://purl.obolibrary.org/obo/GAZ_00051197"/>
        <obo:IAO_0000115>An oasis in Southeastern Libya.</obo:IAO_0000115>
        <oboInOwl:hasOBONamespace>GAZ</oboInOwl:hasOBONamespace>
        <oboInOwl:id>GAZ:00066431</oboInOwl:id>
        <rdfs:label>Kufra Oasis</rdfs:label>
    </owl:NamedIndividual>
    


    <!-- http://purl.obolibrary.org/obo/GAZ_00076687 -->

    <owl:NamedIndividual rdf:about="http://purl.obolibrary.org/obo/GAZ_00076687">
        <obo:RO_0001025 rdf:resource="http://purl.obolibrary.org/obo/GAZ_00000674"/>
        <obo:IAO_0000115>A national park in Sudan. The area lies in the north-eastern corner of the Blue Nile Province adjacent to the frontier with Ethiopia.</obo:IAO_0000115>
        <oboInOwl:hasOBONamespace>GAZ</oboInOwl:hasOBONamespace>
        <oboInOwl:id>GAZ:00076687</oboInOwl:id>
        <rdfs:label>Dinder National Park</rdfs:label>
    </owl:NamedIndividual>
    


    <!-- http://purl.obolibrary.org/obo/GAZ_00076689 -->

    <owl:NamedIndividual rdf:about="http://purl.obolibrary.org/obo/GAZ_00076689">
        <obo:RO_0001025 rdf:resource="http://purl.obolibrary.org/obo/GAZ_00000688"/>
        <obo:IAO_0000115>A national park in Sudan. Located in the south-western corner of southern Darfur Province, 300 km from Nyala, bordering the Central African Republic.</obo:IAO_0000115>
        <oboInOwl:hasOBONamespace>GAZ</oboInOwl:hasOBONamespace>
        <oboInOwl:id>GAZ:00076689</oboInOwl:id>
        <rdfs:label>Radom National Park</rdfs:label>
    </owl:NamedIndividual>
    


    <!-- http://purl.obolibrary.org/obo/GAZ_00089782 -->

    <owl:NamedIndividual rdf:about="http://purl.obolibrary.org/obo/GAZ_00089782">
        <obo:IAO_0000115>Protected areas amounting to 144 islands in different Governorates in Egypt. Alongside the main stream from Aswan until the Barrages, there are 95 Islands within an area of 32500 Feddans. In Rasheed branch there are 30 islands within an area of 3400 Feddans, in Damietta Branch there are 19 islands within and area of 1250 Feddans. The total area of all the Nile River islands in 37150 Feddans.</obo:IAO_0000115>
        <oboInOwl:hasOBONamespace>GAZ</oboInOwl:hasOBONamespace>
        <oboInOwl:id>GAZ:00089782</oboInOwl:id>
        <rdfs:label>Nile river Islands Protected Area</rdfs:label>
    </owl:NamedIndividual>
    


    <!-- http://purl.obolibrary.org/obo/GAZ_00102117 -->

    <owl:NamedIndividual rdf:about="http://purl.obolibrary.org/obo/GAZ_00102117">
        <obo:RO_0001025 rdf:resource="http://purl.obolibrary.org/obo/GAZ_00051269"/>
        <obo:IAO_0000115>The eastern side (3 km wide and 30 m deep) of the Bab-el-Mandeb straits separating Ras Menheli, Yemen, on the Arabian Peninsula and Ras Siyan, Djibouti, on the Horn of Africa. The Yemeni island of Perim divides the strait into two channels.</obo:IAO_0000115>
        <oboInOwl:hasOBONamespace>GAZ</oboInOwl:hasOBONamespace>
        <oboInOwl:id>GAZ:00102117</oboInOwl:id>
        <rdfs:label>Bab Iskender</rdfs:label>
    </owl:NamedIndividual>
    


    <!-- http://purl.obolibrary.org/obo/GAZ_00102118 -->

    <owl:NamedIndividual rdf:about="http://purl.obolibrary.org/obo/GAZ_00102118">
        <obo:RO_0001025 rdf:resource="http://purl.obolibrary.org/obo/GAZ_00051269"/>
        <obo:IAO_0000115>The western side of the Bab-el-Mandeb strait.</obo:IAO_0000115>
        <oboInOwl:hasOBONamespace>GAZ</oboInOwl:hasOBONamespace>
        <oboInOwl:id>GAZ:00102118</oboInOwl:id>
        <rdfs:label>Dact-el-Mayun</rdfs:label>
    </owl:NamedIndividual>
    


    <!-- http://purl.obolibrary.org/obo/GAZ_00103898 -->

    <owl:NamedIndividual rdf:about="http://purl.obolibrary.org/obo/GAZ_00103898">
        <obo:IAO_0000115>A triangular massif, located in northern Niger, within the Sahara desert. Part of the West Saharan montane xeric woodlands ecoregion, they rise to more than 1,830 m and extend over 84000 km2. Lying in the midst of desert north of the 17th parallel, the Air plateau with an average altitude between 500 and 900 m, forms an island of Sahel climate.</obo:IAO_0000115>
        <oboInOwl:hasOBONamespace>GAZ</oboInOwl:hasOBONamespace>
        <oboInOwl:id>GAZ:00103898</oboInOwl:id>
        <rdfs:label>Air Mountains</rdfs:label>
    </owl:NamedIndividual>
    


    <!-- http://purl.obolibrary.org/obo/GAZ_00122801 -->

    <owl:NamedIndividual rdf:about="http://purl.obolibrary.org/obo/GAZ_00122801">
        <obo:IAO_0000115>A depression located at the southern edge of the Sahara Desert in north central Africa, is the lowest point in Chad, and one of the largest sources of airborne dust in the world. Once serving as part of the floor of a much larger Lake Chad.</obo:IAO_0000115>
        <oboInOwl:hasOBONamespace>GAZ</oboInOwl:hasOBONamespace>
        <oboInOwl:id>GAZ:00122801</oboInOwl:id>
        <rdfs:label>Bodele Depression</rdfs:label>
    </owl:NamedIndividual>
    


    <!-- http://purl.obolibrary.org/obo/GAZ_00144637 -->

    <owl:NamedIndividual rdf:about="http://purl.obolibrary.org/obo/GAZ_00144637">
        <obo:RO_0001025 rdf:resource="http://purl.obolibrary.org/obo/GAZ_00002456"/>
        <obo:IAO_0000115>An inlet of water on the Egyptian side of the Red Sea. It is located slightly north of the Tropic of Cancer. The northern part of Foul Bay is the Ras Banas peninsula.</obo:IAO_0000115>
        <oboInOwl:hasOBONamespace>GAZ</oboInOwl:hasOBONamespace>
        <oboInOwl:id>GAZ:00144637</oboInOwl:id>
        <rdfs:label>Foul Bay</rdfs:label>
    </owl:NamedIndividual>
    


    <!-- http://purl.obolibrary.org/obo/GAZ_00144638 -->

    <owl:NamedIndividual rdf:about="http://purl.obolibrary.org/obo/GAZ_00144638">
        <obo:RO_0001025 rdf:resource="http://purl.obolibrary.org/obo/GAZ_00144637"/>
        <obo:IAO_0000115>An island in Foul Bay.</obo:IAO_0000115>
        <oboInOwl:hasOBONamespace>GAZ</oboInOwl:hasOBONamespace>
        <oboInOwl:id>GAZ:00144638</oboInOwl:id>
        <rdfs:label>Rocky Island</rdfs:label>
    </owl:NamedIndividual>
    


    <!-- http://purl.obolibrary.org/obo/GAZ_00144639 -->

    <owl:NamedIndividual rdf:about="http://purl.obolibrary.org/obo/GAZ_00144639">
        <obo:RO_0001025 rdf:resource="http://purl.obolibrary.org/obo/GAZ_00144637"/>
        <obo:IAO_0000115>The largest of a group of islands in Foul Bay, Red Sea in Southern Egypt.</obo:IAO_0000115>
        <oboInOwl:hasOBONamespace>GAZ</oboInOwl:hasOBONamespace>
        <oboInOwl:id>GAZ:00144639</oboInOwl:id>
        <rdfs:label>Saint John&apos;s Island</rdfs:label>
    </owl:NamedIndividual>
    


    <!-- http://purl.obolibrary.org/obo/GAZ_00145311 -->

    <owl:NamedIndividual rdf:about="http://purl.obolibrary.org/obo/GAZ_00145311">
        <obo:RO_0001025 rdf:resource="http://purl.obolibrary.org/obo/GAZ_00002456"/>
        <obo:IAO_0000115>A body of water on the Eritrean coastline on the Red Sea. The Gulf lies near the midpoint of the Eritrean coast, between the Foro province and the Buri Peninsula of the Ghelae&apos;lo province, both in the country&apos;s Northern Red Sea region.</obo:IAO_0000115>
        <oboInOwl:hasOBONamespace>GAZ</oboInOwl:hasOBONamespace>
        <oboInOwl:id>GAZ:00145311</oboInOwl:id>
        <rdfs:label>Gulf of Zula</rdfs:label>
    </owl:NamedIndividual>
    


    <!-- http://purl.obolibrary.org/obo/GAZ_00146201 -->

    <owl:NamedIndividual rdf:about="http://purl.obolibrary.org/obo/GAZ_00146201">
        <obo:RO_0001025 rdf:resource="http://purl.obolibrary.org/obo/GAZ_00002456"/>
        <obo:IAO_0000115>A bay on the Red Sea, off the coast of Eritrea.</obo:IAO_0000115>
        <oboInOwl:hasOBONamespace>GAZ</oboInOwl:hasOBONamespace>
        <oboInOwl:id>GAZ:00146201</oboInOwl:id>
        <rdfs:label>Amphila Bay</rdfs:label>
    </owl:NamedIndividual>
    


    <!-- http://purl.obolibrary.org/obo/GAZ_00176003 -->

    <owl:NamedIndividual rdf:about="http://purl.obolibrary.org/obo/GAZ_00176003">
        <obo:RO_0001025 rdf:resource="http://purl.obolibrary.org/obo/GAZ_00002456"/>
        <obo:IAO_0000115>A small 145 m long and 50 m wide artificial island in the Red Sea at the southern mouth of the Suez Canal.</obo:IAO_0000115>
        <oboInOwl:hasOBONamespace>GAZ</oboInOwl:hasOBONamespace>
        <oboInOwl:id>GAZ:00176003</oboInOwl:id>
        <rdfs:label>Al Jazeera Al Khadraa</rdfs:label>
    </owl:NamedIndividual>
    


    <!-- http://purl.obolibrary.org/obo/GAZ_00176006 -->

    <owl:NamedIndividual rdf:about="http://purl.obolibrary.org/obo/GAZ_00176006">
        <obo:RO_0001025 rdf:resource="http://purl.obolibrary.org/obo/GAZ_00002456"/>
        <obo:IAO_0000115>An island off the coast of Saudi Arabia.</obo:IAO_0000115>
        <oboInOwl:hasOBONamespace>GAZ</oboInOwl:hasOBONamespace>
        <oboInOwl:id>GAZ:00176006</oboInOwl:id>
        <rdfs:label>Saso Island</rdfs:label>
    </owl:NamedIndividual>
    


    <!-- http://purl.obolibrary.org/obo/GAZ_00230302 -->

    <owl:NamedIndividual rdf:about="http://purl.obolibrary.org/obo/GAZ_00230302">
        <obo:RO_0001025 rdf:resource="http://purl.obolibrary.org/obo/GAZ_00009949"/>
        <obo:IAO_0000115>An irrigation canal. Cosntructed 1873.</obo:IAO_0000115>
        <oboInOwl:hasOBONamespace>GAZ</oboInOwl:hasOBONamespace>
        <oboInOwl:id>GAZ:00230302</oboInOwl:id>
        <rdfs:label>Ibrahimiya Canal</rdfs:label>
    </owl:NamedIndividual>
    


    <!-- http://purl.obolibrary.org/obo/GAZ_00230306 -->

    <owl:NamedIndividual rdf:about="http://purl.obolibrary.org/obo/GAZ_00230306">
        <obo:RO_0001025 rdf:resource="http://purl.obolibrary.org/obo/GAZ_00230307"/>
        <obo:IAO_0000115>A mountain range in the area of the Egyptian-Libyan-Sudanese border.</obo:IAO_0000115>
        <oboInOwl:hasOBONamespace>GAZ</oboInOwl:hasOBONamespace>
        <oboInOwl:id>GAZ:00230306</oboInOwl:id>
        <rdfs:label>Jebel Uweinat</rdfs:label>
    </owl:NamedIndividual>
    


    <!-- http://purl.obolibrary.org/obo/GAZ_00230307 -->

    <owl:NamedIndividual rdf:about="http://purl.obolibrary.org/obo/GAZ_00230307">
        <obo:IAO_0000115>A plateau in the remote southwest corner of Egypt.</obo:IAO_0000115>
        <oboInOwl:hasOBONamespace>GAZ</oboInOwl:hasOBONamespace>
        <oboInOwl:id>GAZ:00230307</oboInOwl:id>
        <rdfs:label>Gilf Kebir</rdfs:label>
    </owl:NamedIndividual>
    


    <!-- http://purl.obolibrary.org/obo/GAZ_00230308 -->

    <owl:NamedIndividual rdf:about="http://purl.obolibrary.org/obo/GAZ_00230308">
        <obo:RO_0001025 rdf:resource="http://purl.obolibrary.org/obo/GAZ_00230307"/>
        <obo:IAO_0000115>An impact crater.</obo:IAO_0000115>
        <oboInOwl:hasOBONamespace>GAZ</oboInOwl:hasOBONamespace>
        <oboInOwl:id>GAZ:00230308</oboInOwl:id>
        <rdfs:label>Kebira Crater</rdfs:label>
    </owl:NamedIndividual>
    


    <!-- http://purl.obolibrary.org/obo/GAZ_00230309 -->

    <owl:NamedIndividual rdf:about="http://purl.obolibrary.org/obo/GAZ_00230309">
        <obo:RO_0001025 rdf:resource="http://purl.obolibrary.org/obo/GAZ_00230307"/>
        <obo:IAO_0000115>A dry river bed.</obo:IAO_0000115>
        <oboInOwl:hasOBONamespace>GAZ</oboInOwl:hasOBONamespace>
        <oboInOwl:id>GAZ:00230309</oboInOwl:id>
        <rdfs:label>Wadi Akhdar</rdfs:label>
    </owl:NamedIndividual>
    


    <!-- http://purl.obolibrary.org/obo/GAZ_00230310 -->

    <owl:NamedIndividual rdf:about="http://purl.obolibrary.org/obo/GAZ_00230310">
        <obo:RO_0001025 rdf:resource="http://purl.obolibrary.org/obo/GAZ_00230307"/>
        <obo:IAO_0000115>A dry river bed.</obo:IAO_0000115>
        <oboInOwl:hasOBONamespace>GAZ</oboInOwl:hasOBONamespace>
        <oboInOwl:id>GAZ:00230310</oboInOwl:id>
        <rdfs:label>Wadi Bakht</rdfs:label>
    </owl:NamedIndividual>
    


    <!-- http://purl.obolibrary.org/obo/GAZ_00230311 -->

    <owl:NamedIndividual rdf:about="http://purl.obolibrary.org/obo/GAZ_00230311">
        <obo:RO_0001025 rdf:resource="http://purl.obolibrary.org/obo/GAZ_00230307"/>
        <obo:IAO_0000115>A dry river bed.</obo:IAO_0000115>
        <oboInOwl:hasOBONamespace>GAZ</oboInOwl:hasOBONamespace>
        <oboInOwl:id>GAZ:00230311</oboInOwl:id>
        <rdfs:label>Wadi Dayiq</rdfs:label>
    </owl:NamedIndividual>
    


    <!-- http://purl.obolibrary.org/obo/GAZ_00230312 -->

    <owl:NamedIndividual rdf:about="http://purl.obolibrary.org/obo/GAZ_00230312">
        <obo:RO_0001025 rdf:resource="http://purl.obolibrary.org/obo/GAZ_00230307"/>
        <obo:IAO_0000115>A dry river bed.</obo:IAO_0000115>
        <oboInOwl:hasOBONamespace>GAZ</oboInOwl:hasOBONamespace>
        <oboInOwl:id>GAZ:00230312</oboInOwl:id>
        <rdfs:label>Wadi Firaq</rdfs:label>
    </owl:NamedIndividual>
    


    <!-- http://purl.obolibrary.org/obo/GAZ_00230313 -->

    <owl:NamedIndividual rdf:about="http://purl.obolibrary.org/obo/GAZ_00230313">
        <obo:RO_0001025 rdf:resource="http://purl.obolibrary.org/obo/GAZ_00230307"/>
        <obo:IAO_0000115>A dry river bed.</obo:IAO_0000115>
        <oboInOwl:hasOBONamespace>GAZ</oboInOwl:hasOBONamespace>
        <oboInOwl:id>GAZ:00230313</oboInOwl:id>
        <rdfs:label>Wadi Gazayir</rdfs:label>
    </owl:NamedIndividual>
    


    <!-- http://purl.obolibrary.org/obo/GAZ_00230314 -->

    <owl:NamedIndividual rdf:about="http://purl.obolibrary.org/obo/GAZ_00230314">
        <obo:RO_0001025 rdf:resource="http://purl.obolibrary.org/obo/GAZ_00230307"/>
        <obo:IAO_0000115>A dry river bed.</obo:IAO_0000115>
        <oboInOwl:hasOBONamespace>GAZ</oboInOwl:hasOBONamespace>
        <oboInOwl:id>GAZ:00230314</oboInOwl:id>
        <rdfs:label>Wadi Maftuh</rdfs:label>
    </owl:NamedIndividual>
    


    <!-- http://purl.obolibrary.org/obo/GAZ_00230315 -->

    <owl:NamedIndividual rdf:about="http://purl.obolibrary.org/obo/GAZ_00230315">
        <obo:RO_0001025 rdf:resource="http://purl.obolibrary.org/obo/GAZ_00230307"/>
        <obo:IAO_0000115>A dry river bed.</obo:IAO_0000115>
        <oboInOwl:hasOBONamespace>GAZ</oboInOwl:hasOBONamespace>
        <oboInOwl:id>GAZ:00230315</oboInOwl:id>
        <rdfs:label>Wadi Mashi</rdfs:label>
    </owl:NamedIndividual>
    


    <!-- http://purl.obolibrary.org/obo/GAZ_00230316 -->

    <owl:NamedIndividual rdf:about="http://purl.obolibrary.org/obo/GAZ_00230316">
        <obo:RO_0001025 rdf:resource="http://purl.obolibrary.org/obo/GAZ_00230307"/>
        <obo:IAO_0000115>A dry river bed.</obo:IAO_0000115>
        <oboInOwl:hasOBONamespace>GAZ</oboInOwl:hasOBONamespace>
        <oboInOwl:id>GAZ:00230316</oboInOwl:id>
        <rdfs:label>Wadi Sura</rdfs:label>
    </owl:NamedIndividual>
    


    <!-- http://purl.obolibrary.org/obo/GAZ_00230317 -->

    <owl:NamedIndividual rdf:about="http://purl.obolibrary.org/obo/GAZ_00230317">
        <obo:RO_0001025 rdf:resource="http://purl.obolibrary.org/obo/GAZ_00230307"/>
        <obo:IAO_0000115>A dry river bed.</obo:IAO_0000115>
        <oboInOwl:hasOBONamespace>GAZ</oboInOwl:hasOBONamespace>
        <oboInOwl:id>GAZ:00230317</oboInOwl:id>
        <rdfs:label>Wadi Wassa</rdfs:label>
    </owl:NamedIndividual>
    


    <!-- http://purl.obolibrary.org/obo/GAZ_00230323 -->

    <owl:NamedIndividual rdf:about="http://purl.obolibrary.org/obo/GAZ_00230323">
        <obo:RO_0001025 rdf:resource="http://purl.obolibrary.org/obo/GAZ_00230307"/>
        <obo:IAO_0000115>A cave in southwest Egypt, near the border with Libya, in the mountainous Gilf Kebir region of the Sahara Desert.</obo:IAO_0000115>
        <oboInOwl:hasOBONamespace>GAZ</oboInOwl:hasOBONamespace>
        <oboInOwl:id>GAZ:00230323</oboInOwl:id>
        <rdfs:label>Cave of Swimmers</rdfs:label>
    </owl:NamedIndividual>
    


    <!-- http://purl.obolibrary.org/obo/GAZ_00230324 -->

    <owl:NamedIndividual rdf:about="http://purl.obolibrary.org/obo/GAZ_00230324">
        <obo:RO_0001025 rdf:resource="http://purl.obolibrary.org/obo/GAZ_00058890"/>
        <obo:IAO_0000115>An island in the first cataract of the Nile River, Egypt.</obo:IAO_0000115>
        <oboInOwl:hasOBONamespace>GAZ</oboInOwl:hasOBONamespace>
        <oboInOwl:id>GAZ:00230324</oboInOwl:id>
        <rdfs:label>Bigeh</rdfs:label>
    </owl:NamedIndividual>
    


    <!-- http://purl.obolibrary.org/obo/GAZ_00230325 -->

    <owl:NamedIndividual rdf:about="http://purl.obolibrary.org/obo/GAZ_00230325">
        <obo:IAO_0000115>An island in the River Nile, located just downstream of the First Cataract.</obo:IAO_0000115>
        <oboInOwl:hasOBONamespace>GAZ</oboInOwl:hasOBONamespace>
        <oboInOwl:id>GAZ:00230325</oboInOwl:id>
        <rdfs:label>Elephantine</rdfs:label>
    </owl:NamedIndividual>
    


    <!-- http://purl.obolibrary.org/obo/GAZ_00230326 -->

    <owl:NamedIndividual rdf:about="http://purl.obolibrary.org/obo/GAZ_00230326">
        <obo:IAO_0000115>An island located in the Nile River, in central Cairo.</obo:IAO_0000115>
        <oboInOwl:hasOBONamespace>GAZ</oboInOwl:hasOBONamespace>
        <oboInOwl:id>GAZ:00230326</oboInOwl:id>
        <rdfs:label>Gezira Island</rdfs:label>
    </owl:NamedIndividual>
    


    <!-- http://purl.obolibrary.org/obo/GAZ_00230327 -->

    <owl:NamedIndividual rdf:about="http://purl.obolibrary.org/obo/GAZ_00230327">
        <obo:IAO_0000115>An oval-shaped island in the Nile at Aswan, Egypt.</obo:IAO_0000115>
        <oboInOwl:hasOBONamespace>GAZ</oboInOwl:hasOBONamespace>
        <oboInOwl:id>GAZ:00230327</oboInOwl:id>
        <rdfs:label>Geziret an-Nabatat</rdfs:label>
    </owl:NamedIndividual>
    


    <!-- http://purl.obolibrary.org/obo/GAZ_00230337 -->

    <owl:NamedIndividual rdf:about="http://purl.obolibrary.org/obo/GAZ_00230337">
        <oboInOwl:hasOBONamespace>GAZ</oboInOwl:hasOBONamespace>
        <oboInOwl:id>GAZ:00230337</oboInOwl:id>
        <rdfs:label>Sarana River</rdfs:label>
    </owl:NamedIndividual>
    


    <!-- http://purl.obolibrary.org/obo/GAZ_00230338 -->

    <owl:NamedIndividual rdf:about="http://purl.obolibrary.org/obo/GAZ_00230338">
        <oboInOwl:hasOBONamespace>GAZ</oboInOwl:hasOBONamespace>
        <oboInOwl:id>GAZ:00230338</oboInOwl:id>
        <rdfs:label>Balasa River</rdfs:label>
    </owl:NamedIndividual>
    


    <!-- http://purl.obolibrary.org/obo/GAZ_00230339 -->

    <owl:NamedIndividual rdf:about="http://purl.obolibrary.org/obo/GAZ_00230339">
        <obo:IAO_0000115>A river. A tributary of the Mareb River in Ethiopia.</obo:IAO_0000115>
        <oboInOwl:hasOBONamespace>GAZ</oboInOwl:hasOBONamespace>
        <oboInOwl:id>GAZ:00230339</oboInOwl:id>
        <rdfs:label>Mai Shawesh River</rdfs:label>
    </owl:NamedIndividual>
    


    <!-- http://purl.obolibrary.org/obo/GAZ_00230340 -->

    <owl:NamedIndividual rdf:about="http://purl.obolibrary.org/obo/GAZ_00230340">
        <obo:IAO_0000115>A river. A tributary of the Mareb River in Ethiopia.</obo:IAO_0000115>
        <oboInOwl:hasOBONamespace>GAZ</oboInOwl:hasOBONamespace>
        <oboInOwl:id>GAZ:00230340</oboInOwl:id>
        <rdfs:label>&apos;Engweya River</rdfs:label>
    </owl:NamedIndividual>
    


    <!-- http://purl.obolibrary.org/obo/GAZ_00230398 -->

    <owl:NamedIndividual rdf:about="http://purl.obolibrary.org/obo/GAZ_00230398">
        <obo:IAO_0000115>A river. A tributary of the Jamma River. Along with the Adabay River, it defined the border of the former district of Marra Biete.</obo:IAO_0000115>
        <oboInOwl:hasOBONamespace>GAZ</oboInOwl:hasOBONamespace>
        <oboInOwl:id>GAZ:00230398</oboInOwl:id>
        <rdfs:label>Wanchet River</rdfs:label>
    </owl:NamedIndividual>
    


    <!-- http://purl.obolibrary.org/obo/GAZ_00230400 -->

    <owl:NamedIndividual rdf:about="http://purl.obolibrary.org/obo/GAZ_00230400">
        <obo:IAO_0000115>A river in Sudan, Africa. The most southerly of the great eastern tributaries of the Nile, the Sobat enters the White Nile at Dolieb Hill, near the city of Malakal in the Upper Nile state of Sudan.</obo:IAO_0000115>
        <oboInOwl:hasOBONamespace>GAZ</oboInOwl:hasOBONamespace>
        <oboInOwl:id>GAZ:00230400</oboInOwl:id>
        <rdfs:label>Sobat River</rdfs:label>
    </owl:NamedIndividual>
    


    <!-- http://purl.obolibrary.org/obo/GAZ_00230410 -->

    <owl:NamedIndividual rdf:about="http://purl.obolibrary.org/obo/GAZ_00230410">
        <obo:IAO_0000115>A river of southwestern Ethiopia. It is a tributary of the Baro River.</obo:IAO_0000115>
        <oboInOwl:hasOBONamespace>GAZ</oboInOwl:hasOBONamespace>
        <oboInOwl:id>GAZ:00230410</oboInOwl:id>
        <rdfs:label>Jikawo River</rdfs:label>
    </owl:NamedIndividual>
    


    <!-- http://purl.obolibrary.org/obo/GAZ_00230416 -->

    <owl:NamedIndividual rdf:about="http://purl.obolibrary.org/obo/GAZ_00230416">
        <obo:IAO_0000115>A dam. Constructed 1986.</obo:IAO_0000115>
        <oboInOwl:hasOBONamespace>GAZ</oboInOwl:hasOBONamespace>
        <oboInOwl:id>GAZ:00230416</oboInOwl:id>
        <rdfs:label>Angereb Dam</rdfs:label>
    </owl:NamedIndividual>
    


    <!-- http://purl.obolibrary.org/obo/GAZ_00230530 -->

    <owl:NamedIndividual rdf:about="http://purl.obolibrary.org/obo/GAZ_00230530">
        <obo:IAO_0000115>A valley in west-central Libya, arising out of the Sawda Mountains, situated between the towns Wanzarik and Umm al-&apos;Abid in the west and east, respectively.</obo:IAO_0000115>
        <oboInOwl:hasOBONamespace>GAZ</oboInOwl:hasOBONamespace>
        <oboInOwl:id>GAZ:00230530</oboInOwl:id>
        <rdfs:label>Wadi ash-Shati&apos;</rdfs:label>
    </owl:NamedIndividual>
    


    <!-- http://purl.obolibrary.org/obo/GAZ_00230531 -->

    <owl:NamedIndividual rdf:about="http://purl.obolibrary.org/obo/GAZ_00230531">
        <obo:IAO_0000115>A primarily erg desert in southwestern Libya and is considered part of the Sahara desert complex, although it is separated from the southern Sahara by the Tibesti Mountains and the Tassili n&apos;Ajjer.</obo:IAO_0000115>
        <oboInOwl:hasOBONamespace>GAZ</oboInOwl:hasOBONamespace>
        <oboInOwl:id>GAZ:00230531</oboInOwl:id>
        <rdfs:label>Murzuq Desert</rdfs:label>
    </owl:NamedIndividual>
    


    <!-- http://purl.obolibrary.org/obo/GAZ_00230545 -->

    <owl:NamedIndividual rdf:about="http://purl.obolibrary.org/obo/GAZ_00230545">
        <obo:IAO_0000115>An erg located in the far south-east of Western Sahara.</obo:IAO_0000115>
        <oboInOwl:hasOBONamespace>GAZ</oboInOwl:hasOBONamespace>
        <oboInOwl:id>GAZ:00230545</oboInOwl:id>
        <rdfs:label>Zug</rdfs:label>
    </owl:NamedIndividual>
    


    <!-- http://purl.obolibrary.org/obo/GAZ_00230712 -->

    <owl:NamedIndividual rdf:about="http://purl.obolibrary.org/obo/GAZ_00230712">
        <obo:IAO_0000115>A sandstone massif in Mali&apos;s Kidal Region.</obo:IAO_0000115>
        <oboInOwl:hasOBONamespace>GAZ</oboInOwl:hasOBONamespace>
        <oboInOwl:id>GAZ:00230712</oboInOwl:id>
        <rdfs:label>Adrar des Ifoghas</rdfs:label>
    </owl:NamedIndividual>
    


    <!-- http://purl.obolibrary.org/obo/GAZ_00231580 -->

    <owl:NamedIndividual rdf:about="http://purl.obolibrary.org/obo/GAZ_00231580">
        <obo:IAO_0000115>A plateau that lies in eastern Mauritania, forming a stony part of the Sahara Desert.</obo:IAO_0000115>
        <oboInOwl:hasOBONamespace>GAZ</oboInOwl:hasOBONamespace>
        <oboInOwl:id>GAZ:00231580</oboInOwl:id>
        <rdfs:label>Tagant Plateau</rdfs:label>
    </owl:NamedIndividual>
    


    <!-- http://purl.obolibrary.org/obo/GAZ_00231625 -->

    <owl:NamedIndividual rdf:about="http://purl.obolibrary.org/obo/GAZ_00231625">
        <obo:IAO_0000115>A highland area of the Sahara Desert in northern Mauritania.</obo:IAO_0000115>
        <oboInOwl:hasOBONamespace>GAZ</oboInOwl:hasOBONamespace>
        <oboInOwl:id>GAZ:00231625</oboInOwl:id>
        <rdfs:label>Adrar Plateau</rdfs:label>
    </owl:NamedIndividual>
    


    <!-- http://purl.obolibrary.org/obo/GAZ_00233408 -->

    <owl:NamedIndividual rdf:about="http://purl.obolibrary.org/obo/GAZ_00233408">
        <obo:IAO_0000115>A protected area. Established 1988-01-01.</obo:IAO_0000115>
        <oboInOwl:hasOBONamespace>GAZ</oboInOwl:hasOBONamespace>
        <oboInOwl:id>GAZ:00233408</oboInOwl:id>
        <rdfs:label>Air and Tenere Addax Sanctuary</rdfs:label>
    </owl:NamedIndividual>
    


    <!-- http://purl.obolibrary.org/obo/GAZ_00233409 -->

    <owl:NamedIndividual rdf:about="http://purl.obolibrary.org/obo/GAZ_00233409">
        <obo:IAO_0000115>A protected area. It includes both the eastern half of the Air Mountains and the western sections of the Tenere desert.</obo:IAO_0000115>
        <oboInOwl:hasOBONamespace>GAZ</oboInOwl:hasOBONamespace>
        <oboInOwl:id>GAZ:00233409</oboInOwl:id>
        <rdfs:label>Air and Tenere National Nature Reserve</rdfs:label>
    </owl:NamedIndividual>
    


    <!-- http://purl.obolibrary.org/obo/GAZ_00233411 -->

    <owl:NamedIndividual rdf:about="http://purl.obolibrary.org/obo/GAZ_00233411">
        <obo:IAO_0000115>A plateau that ies in the Sahara, in north eastern Niger.</obo:IAO_0000115>
        <oboInOwl:hasOBONamespace>GAZ</oboInOwl:hasOBONamespace>
        <oboInOwl:id>GAZ:00233411</oboInOwl:id>
        <rdfs:label>Djado Plateau</rdfs:label>
    </owl:NamedIndividual>
    


    <!-- http://purl.obolibrary.org/obo/GAZ_00233412 -->

    <owl:NamedIndividual rdf:about="http://purl.obolibrary.org/obo/GAZ_00233412">
        <obo:RO_0001025 rdf:resource="http://purl.obolibrary.org/obo/GAZ_00103898"/>
        <obo:RO_0001025 rdf:resource="http://purl.obolibrary.org/obo/GAZ_00233408"/>
        <obo:IAO_0000115>A mountain range in Niger in the northeastern section of the Air Massif, about 100 km ENE of the town of Iferouane and 30 km NE of the Tezerik oasis. Isolated from the main Massif by dune seas of the Erg of Tenere and a flat gravely Desert pavement plain.</obo:IAO_0000115>
        <oboInOwl:hasOBONamespace>GAZ</oboInOwl:hasOBONamespace>
        <oboInOwl:id>GAZ:00233412</oboInOwl:id>
        <rdfs:label>Montagnes Bleus</rdfs:label>
    </owl:NamedIndividual>
    


    <!-- http://purl.obolibrary.org/obo/GAZ_00233432 -->

    <owl:NamedIndividual rdf:about="http://purl.obolibrary.org/obo/GAZ_00233432">
        <obo:RO_0001025 rdf:resource="http://purl.obolibrary.org/obo/GAZ_00051198"/>
        <obo:IAO_0000115>An oasis surrounded by the Tenere dessert and the dunes of the Erg of Bilma in eastern Niger, placed on the western edge of the small Agram mountain outcropping.</obo:IAO_0000115>
        <oboInOwl:hasOBONamespace>GAZ</oboInOwl:hasOBONamespace>
        <oboInOwl:id>GAZ:00233432</oboInOwl:id>
        <rdfs:label>Fachi</rdfs:label>
    </owl:NamedIndividual>
    


    <!-- http://purl.obolibrary.org/obo/GAZ_00233440 -->

    <owl:NamedIndividual rdf:about="http://purl.obolibrary.org/obo/GAZ_00233440">
        <obo:RO_0001025 rdf:resource="http://purl.obolibrary.org/obo/GAZ_00000689"/>
        <obo:IAO_0000115>Mountains.</obo:IAO_0000115>
        <oboInOwl:hasOBONamespace>GAZ</oboInOwl:hasOBONamespace>
        <oboInOwl:id>GAZ:00233440</oboInOwl:id>
        <rdfs:label>Nuba Mountains</rdfs:label>
    </owl:NamedIndividual>
    


    <!-- http://purl.obolibrary.org/obo/GAZ_00233441 -->

    <owl:NamedIndividual rdf:about="http://purl.obolibrary.org/obo/GAZ_00233441">
        <obo:RO_0001025 rdf:resource="http://purl.obolibrary.org/obo/GAZ_00000560"/>
        <obo:IAO_0000115>One of the two semi-autonomous areas of Sudan.</obo:IAO_0000115>
        <oboInOwl:hasOBONamespace>GAZ</oboInOwl:hasOBONamespace>
        <oboInOwl:id>GAZ:00233441</oboInOwl:id>
        <rdfs:label>Northern Sudan</rdfs:label>
    </owl:NamedIndividual>
    


    <!-- http://purl.obolibrary.org/obo/GAZ_00233534 -->

    <owl:NamedIndividual rdf:about="http://purl.obolibrary.org/obo/GAZ_00233534">
        <obo:IAO_0000115>A lake. Formed by a widening of the channel of the Bahr el Ghazal.</obo:IAO_0000115>
        <oboInOwl:hasOBONamespace>GAZ</oboInOwl:hasOBONamespace>
        <oboInOwl:id>GAZ:00233534</oboInOwl:id>
        <rdfs:label>Lake Ambadi</rdfs:label>
    </owl:NamedIndividual>
    


    <!-- http://purl.obolibrary.org/obo/GAZ_00233536 -->

    <owl:NamedIndividual rdf:about="http://purl.obolibrary.org/obo/GAZ_00233536">
        <obo:RO_0001025 rdf:resource="http://purl.obolibrary.org/obo/GAZ_00000687"/>
        <obo:IAO_0000115>A dam on the Blue Nile near the town of Sennar, Sudan. Constructed 1925.</obo:IAO_0000115>
        <oboInOwl:hasOBONamespace>GAZ</oboInOwl:hasOBONamespace>
        <oboInOwl:id>GAZ:00233536</oboInOwl:id>
        <rdfs:label>Sennar Dam</rdfs:label>
    </owl:NamedIndividual>
    


    <!-- http://purl.obolibrary.org/obo/GAZ_00233537 -->

    <owl:NamedIndividual rdf:about="http://purl.obolibrary.org/obo/GAZ_00233537">
        <obo:RO_0001025 rdf:resource="http://purl.obolibrary.org/obo/GAZ_00000674"/>
        <obo:IAO_0000115>A hydroelectric dam. Impounds El Roseires Lake. Completed 1966.</obo:IAO_0000115>
        <oboInOwl:hasOBONamespace>GAZ</oboInOwl:hasOBONamespace>
        <oboInOwl:id>GAZ:00233537</oboInOwl:id>
        <rdfs:label>El Roseires Dam</rdfs:label>
    </owl:NamedIndividual>
    


    <!-- http://purl.obolibrary.org/obo/GAZ_00233538 -->

    <owl:NamedIndividual rdf:about="http://purl.obolibrary.org/obo/GAZ_00233538">
        <obo:RO_0001025 rdf:resource="http://purl.obolibrary.org/obo/GAZ_00032307"/>
        <obo:IAO_0000115>The capital of Sudan and of Khartoum State. It is located at the confluence of the White Nile flowing north from Lake Victoria, and the Blue Nile flowing west from Ethiopia.</obo:IAO_0000115>
        <oboInOwl:hasOBONamespace>GAZ</oboInOwl:hasOBONamespace>
        <oboInOwl:id>GAZ:00233538</oboInOwl:id>
        <rdfs:label>Khartoum</rdfs:label>
    </owl:NamedIndividual>
    


    <!-- http://purl.obolibrary.org/obo/GAZ_00233539 -->

    <owl:NamedIndividual rdf:about="http://purl.obolibrary.org/obo/GAZ_00233539">
        <obo:RO_0001025 rdf:resource="http://purl.obolibrary.org/obo/GAZ_00000684"/>
        <obo:IAO_0000115>A low lying area by the Nile in Sudan. Located just below the Third Cataract it is the largest section of flood plain on the Donogola Reach.</obo:IAO_0000115>
        <oboInOwl:hasOBONamespace>GAZ</oboInOwl:hasOBONamespace>
        <oboInOwl:id>GAZ:00233539</oboInOwl:id>
        <rdfs:label>Kerma Basin</rdfs:label>
    </owl:NamedIndividual>
    


    <!-- http://purl.obolibrary.org/obo/GAZ_00233540 -->

    <owl:NamedIndividual rdf:about="http://purl.obolibrary.org/obo/GAZ_00233540">
        <obo:IAO_0000115>An island on the White Nile to the south of Khartoum, Sudan.</obo:IAO_0000115>
        <oboInOwl:hasOBONamespace>GAZ</oboInOwl:hasOBONamespace>
        <oboInOwl:id>GAZ:00233540</oboInOwl:id>
        <rdfs:label>Aba Island</rdfs:label>
    </owl:NamedIndividual>
    


    <!-- http://purl.obolibrary.org/obo/GAZ_00233541 -->

    <owl:NamedIndividual rdf:about="http://purl.obolibrary.org/obo/GAZ_00233541">
        <obo:RO_0001025 rdf:resource="http://purl.obolibrary.org/obo/GAZ_00000684"/>
        <obo:IAO_0000115>One of the biggest islands in the Nile and the second biggest island in Sudan. It is 56 km Northern to Dongola the capital of the Northern State in Sudan.</obo:IAO_0000115>
        <oboInOwl:hasOBONamespace>GAZ</oboInOwl:hasOBONamespace>
        <oboInOwl:id>GAZ:00233541</oboInOwl:id>
        <rdfs:label>Badien Island</rdfs:label>
    </owl:NamedIndividual>
    


    <!-- http://purl.obolibrary.org/obo/GAZ_00233542 -->

    <owl:NamedIndividual rdf:about="http://purl.obolibrary.org/obo/GAZ_00233542">
        <obo:RO_0001025 rdf:resource="http://purl.obolibrary.org/obo/GAZ_00000684"/>
        <obo:IAO_0000115>A large island in the Nile River in Nubia between the second and third cataracts. It is 12 km long and 5.5 km wide.</obo:IAO_0000115>
        <oboInOwl:hasOBONamespace>GAZ</oboInOwl:hasOBONamespace>
        <oboInOwl:id>GAZ:00233542</oboInOwl:id>
        <rdfs:label>Sai</rdfs:label>
    </owl:NamedIndividual>
    


    <!-- http://purl.obolibrary.org/obo/GAZ_00233543 -->

    <owl:NamedIndividual rdf:about="http://purl.obolibrary.org/obo/GAZ_00233543">
        <obo:IAO_0000115>An island in Sudan where the White Nile and Blue Nile merge to form the main Nile. It is surrounded by Khartoum, Omdurman and Khartoum North.</obo:IAO_0000115>
        <oboInOwl:hasOBONamespace>GAZ</oboInOwl:hasOBONamespace>
        <oboInOwl:id>GAZ:00233543</oboInOwl:id>
        <rdfs:label>Tuti Island</rdfs:label>
    </owl:NamedIndividual>
    


    <!-- http://purl.obolibrary.org/obo/GAZ_00233583 -->

    <owl:NamedIndividual rdf:about="http://purl.obolibrary.org/obo/GAZ_00233583">
        <oboInOwl:hasOBONamespace>GAZ</oboInOwl:hasOBONamespace>
        <oboInOwl:id>GAZ:00233583</oboInOwl:id>
        <rdfs:label>Schott Dscherid</rdfs:label>
    </owl:NamedIndividual>
    


    <!-- http://purl.obolibrary.org/obo/GAZ_00237174 -->

    <owl:NamedIndividual rdf:about="http://purl.obolibrary.org/obo/GAZ_00237174">
        <obo:IAO_0000115>A hydroelectric power station across the White Nile near to its source at Lake Victoria in Uganda.</obo:IAO_0000115>
        <oboInOwl:hasOBONamespace>GAZ</oboInOwl:hasOBONamespace>
        <oboInOwl:id>GAZ:00237174</oboInOwl:id>
        <rdfs:label>Nalubaale Power Station</rdfs:label>
    </owl:NamedIndividual>
    


    <!-- http://purl.obolibrary.org/obo/GAZ_00237175 -->

    <owl:NamedIndividual rdf:about="http://purl.obolibrary.org/obo/GAZ_00237175">
        <obo:IAO_0000115>A hydroelectric power station located in Jinja, Jinja District, in eastern central Uganda.</obo:IAO_0000115>
        <oboInOwl:hasOBONamespace>GAZ</oboInOwl:hasOBONamespace>
        <oboInOwl:id>GAZ:00237175</oboInOwl:id>
        <rdfs:label>Kiira Power Station</rdfs:label>
    </owl:NamedIndividual>
    


    <!-- http://purl.obolibrary.org/obo/GAZ_00237176 -->

    <owl:NamedIndividual rdf:about="http://purl.obolibrary.org/obo/GAZ_00237176">
        <obo:IAO_0000115>A hydroelectric power project located at the headwaters of River Nile, about 16 km north of Jinja at the former location of Bujagali Falls.</obo:IAO_0000115>
        <oboInOwl:hasOBONamespace>GAZ</oboInOwl:hasOBONamespace>
        <oboInOwl:id>GAZ:00237176</oboInOwl:id>
        <rdfs:label>Bujagali Power Station</rdfs:label>
    </owl:NamedIndividual>
    


    <!-- http://purl.obolibrary.org/obo/GAZ_00237412 -->

    <owl:NamedIndividual rdf:about="http://purl.obolibrary.org/obo/GAZ_00237412">
        <obo:IAO_0000115>A river of eastern Uganda in eastern Africa. It flows in a southern and south-westerly direction and eventually via the Okere River reaches Lake Kyoga.</obo:IAO_0000115>
        <oboInOwl:hasOBONamespace>GAZ</oboInOwl:hasOBONamespace>
        <oboInOwl:id>GAZ:00237412</oboInOwl:id>
        <rdfs:label>Okot River</rdfs:label>
    </owl:NamedIndividual>
    


    <!-- http://purl.obolibrary.org/obo/GAZ_00246604 -->

    <owl:NamedIndividual rdf:about="http://purl.obolibrary.org/obo/GAZ_00246604">
        <obo:IAO_0000115>A freshwater lake. One of the most isolated occurrences of free surface water in the Sahara. It is situated near the southwestern extremity of the plateau, Adrar Nahalet, which extends westwards from the massif of the A&apos;Haggar. The permanent guelta (pool), 13 m wide when full and 6 m deep, is inside a volcanic crater which partly encloses a valley. It collects water from two oueds which drain Ziza Mountain, to the south, and is reputed to have no underground input. Several small temporary pools also occur in the bed of the main oued draining Mount Ziza.</obo:IAO_0000115>
        <oboInOwl:hasOBONamespace>GAZ</oboInOwl:hasOBONamespace>
        <oboInOwl:id>GAZ:00246604</oboInOwl:id>
        <rdfs:label>Gueltas of Ziza</rdfs:label>
    </owl:NamedIndividual>
    


    <!-- http://purl.obolibrary.org/obo/GAZ_00247178 -->

    <owl:NamedIndividual rdf:about="http://purl.obolibrary.org/obo/GAZ_00247178">
        <obo:IAO_0000115>A depression.</obo:IAO_0000115>
        <oboInOwl:hasOBONamespace>GAZ</oboInOwl:hasOBONamespace>
        <oboInOwl:id>GAZ:00247178</oboInOwl:id>
        <rdfs:label>Depression du Mourdi</rdfs:label>
    </owl:NamedIndividual>
    


    <!-- http://purl.obolibrary.org/obo/GAZ_00247180 -->

    <owl:NamedIndividual rdf:about="http://purl.obolibrary.org/obo/GAZ_00247180">
        <obo:IAO_0000115>A mountain range.</obo:IAO_0000115>
        <oboInOwl:hasOBONamespace>GAZ</oboInOwl:hasOBONamespace>
        <oboInOwl:id>GAZ:00247180</oboInOwl:id>
        <rdfs:label>Massif du Kerkour Nourene</rdfs:label>
    </owl:NamedIndividual>
    


    <!-- http://purl.obolibrary.org/obo/GAZ_00247676 -->

    <owl:NamedIndividual rdf:about="http://purl.obolibrary.org/obo/GAZ_00247676">
        <obo:IAO_0000115>An intermittent river in the Sahara.</obo:IAO_0000115>
        <oboInOwl:hasOBONamespace>GAZ</oboInOwl:hasOBONamespace>
        <oboInOwl:id>GAZ:00247676</oboInOwl:id>
        <rdfs:label>Oued Saoura</rdfs:label>
    </owl:NamedIndividual>
    


    <!-- http://purl.obolibrary.org/obo/GAZ_00247997 -->

    <owl:NamedIndividual rdf:about="http://purl.obolibrary.org/obo/GAZ_00247997">
        <obo:RO_0001025 rdf:resource="http://purl.obolibrary.org/obo/GAZ_00009949"/>
        <obo:IAO_0000115>A lake.</obo:IAO_0000115>
        <oboInOwl:hasOBONamespace>GAZ</oboInOwl:hasOBONamespace>
        <oboInOwl:id>GAZ:00247997</oboInOwl:id>
        <rdfs:label>Birkat al Mallah</rdfs:label>
    </owl:NamedIndividual>
    


    <!-- http://purl.obolibrary.org/obo/GAZ_00247998 -->

    <owl:NamedIndividual rdf:about="http://purl.obolibrary.org/obo/GAZ_00247998">
        <obo:RO_0001025 rdf:resource="http://purl.obolibrary.org/obo/GAZ_00009949"/>
        <obo:IAO_0000115>A lake.</obo:IAO_0000115>
        <oboInOwl:hasOBONamespace>GAZ</oboInOwl:hasOBONamespace>
        <oboInOwl:id>GAZ:00247998</oboInOwl:id>
        <rdfs:label>Birkat al Qatta</rdfs:label>
    </owl:NamedIndividual>
    


    <!-- http://purl.obolibrary.org/obo/GAZ_00247999 -->

    <owl:NamedIndividual rdf:about="http://purl.obolibrary.org/obo/GAZ_00247999">
        <obo:RO_0001025 rdf:resource="http://purl.obolibrary.org/obo/GAZ_00009949"/>
        <obo:IAO_0000115>A lake.</obo:IAO_0000115>
        <oboInOwl:hasOBONamespace>GAZ</oboInOwl:hasOBONamespace>
        <oboInOwl:id>GAZ:00247999</oboInOwl:id>
        <rdfs:label>Lake Faraontya</rdfs:label>
    </owl:NamedIndividual>
    


    <!-- http://purl.obolibrary.org/obo/GAZ_00248000 -->

    <owl:NamedIndividual rdf:about="http://purl.obolibrary.org/obo/GAZ_00248000">
        <obo:RO_0001025 rdf:resource="http://purl.obolibrary.org/obo/GAZ_00009949"/>
        <obo:IAO_0000115>A coastal lagoon.</obo:IAO_0000115>
        <oboInOwl:hasOBONamespace>GAZ</oboInOwl:hasOBONamespace>
        <oboInOwl:id>GAZ:00248000</oboInOwl:id>
        <rdfs:label>Buhayrat al Manzilah</rdfs:label>
    </owl:NamedIndividual>
    


    <!-- http://purl.obolibrary.org/obo/GAZ_00248001 -->

    <owl:NamedIndividual rdf:about="http://purl.obolibrary.org/obo/GAZ_00248001">
        <obo:RO_0001025 rdf:resource="http://purl.obolibrary.org/obo/GAZ_00009949"/>
        <obo:IAO_0000115>A lake.</obo:IAO_0000115>
        <oboInOwl:hasOBONamespace>GAZ</oboInOwl:hasOBONamespace>
        <oboInOwl:id>GAZ:00248001</oboInOwl:id>
        <rdfs:label>Birkat Muhayshir</rdfs:label>
    </owl:NamedIndividual>
    


    <!-- http://purl.obolibrary.org/obo/GAZ_00248005 -->

    <owl:NamedIndividual rdf:about="http://purl.obolibrary.org/obo/GAZ_00248005">
        <obo:RO_0001025 rdf:resource="http://purl.obolibrary.org/obo/GAZ_00002456"/>
        <obo:IAO_0000115>An island offshore Al Ghardaqah.</obo:IAO_0000115>
        <oboInOwl:hasOBONamespace>GAZ</oboInOwl:hasOBONamespace>
        <oboInOwl:id>GAZ:00248005</oboInOwl:id>
        <rdfs:label>Abu Minciar Island</rdfs:label>
    </owl:NamedIndividual>
    


    <!-- http://purl.obolibrary.org/obo/GAZ_00248006 -->

    <owl:NamedIndividual rdf:about="http://purl.obolibrary.org/obo/GAZ_00248006">
        <obo:RO_0001025 rdf:resource="http://purl.obolibrary.org/obo/GAZ_00002456"/>
        <obo:IAO_0000115>An island offshore Port Sataga.</obo:IAO_0000115>
        <oboInOwl:hasOBONamespace>GAZ</oboInOwl:hasOBONamespace>
        <oboInOwl:id>GAZ:00248006</oboInOwl:id>
        <rdfs:label>Safaga Island</rdfs:label>
    </owl:NamedIndividual>
    


    <!-- http://purl.obolibrary.org/obo/GAZ_00248007 -->

    <owl:NamedIndividual rdf:about="http://purl.obolibrary.org/obo/GAZ_00248007">
        <obo:RO_0001025 rdf:resource="http://purl.obolibrary.org/obo/GAZ_00002456"/>
        <obo:IAO_0000115>An island.</obo:IAO_0000115>
        <oboInOwl:hasOBONamespace>GAZ</oboInOwl:hasOBONamespace>
        <oboInOwl:id>GAZ:00248007</oboInOwl:id>
        <rdfs:label>Jazirat Wadi Jimal</rdfs:label>
    </owl:NamedIndividual>
    


    <!-- http://purl.obolibrary.org/obo/GAZ_00248009 -->

    <owl:NamedIndividual rdf:about="http://purl.obolibrary.org/obo/GAZ_00248009">
        <obo:RO_0001025 rdf:resource="http://purl.obolibrary.org/obo/GAZ_00051197"/>
        <obo:IAO_0000115>A depression, about 25 m below sea level at its deepest. Bounded by steep slopes on the northern side, reaching about 120-160 m asl, but by much gentler slopes to the south and southeast.</obo:IAO_0000115>
        <oboInOwl:hasOBONamespace>GAZ</oboInOwl:hasOBONamespace>
        <oboInOwl:id>GAZ:00248009</oboInOwl:id>
        <rdfs:label>Siwa Depression</rdfs:label>
    </owl:NamedIndividual>
    


    <!-- http://purl.obolibrary.org/obo/GAZ_00248010 -->

    <owl:NamedIndividual rdf:about="http://purl.obolibrary.org/obo/GAZ_00248010">
        <obo:RO_0001025 rdf:resource="http://purl.obolibrary.org/obo/GAZ_00248009"/>
        <obo:IAO_0000115>An oasis.</obo:IAO_0000115>
        <oboInOwl:hasOBONamespace>GAZ</oboInOwl:hasOBONamespace>
        <oboInOwl:id>GAZ:00248010</oboInOwl:id>
        <rdfs:label>Shiyata</rdfs:label>
    </owl:NamedIndividual>
    


    <!-- http://purl.obolibrary.org/obo/GAZ_00248011 -->

    <owl:NamedIndividual rdf:about="http://purl.obolibrary.org/obo/GAZ_00248011">
        <obo:RO_0001025 rdf:resource="http://purl.obolibrary.org/obo/GAZ_00248009"/>
        <obo:IAO_0000115>A saline lake.</obo:IAO_0000115>
        <oboInOwl:hasOBONamespace>GAZ</oboInOwl:hasOBONamespace>
        <oboInOwl:id>GAZ:00248011</oboInOwl:id>
        <rdfs:label>Birkat al Maraqi</rdfs:label>
    </owl:NamedIndividual>
    


    <!-- http://purl.obolibrary.org/obo/GAZ_00248012 -->

    <owl:NamedIndividual rdf:about="http://purl.obolibrary.org/obo/GAZ_00248012">
        <obo:RO_0001025 rdf:resource="http://purl.obolibrary.org/obo/GAZ_00248009"/>
        <obo:IAO_0000115>A saline lake.</obo:IAO_0000115>
        <oboInOwl:hasOBONamespace>GAZ</oboInOwl:hasOBONamespace>
        <oboInOwl:id>GAZ:00248012</oboInOwl:id>
        <rdfs:label>Birkat el Zaytun</rdfs:label>
    </owl:NamedIndividual>
    


    <!-- http://purl.obolibrary.org/obo/GAZ_00248013 -->

    <owl:NamedIndividual rdf:about="http://purl.obolibrary.org/obo/GAZ_00248013">
        <obo:RO_0001025 rdf:resource="http://purl.obolibrary.org/obo/GAZ_00248009"/>
        <obo:IAO_0000115>A saline lake.</obo:IAO_0000115>
        <oboInOwl:hasOBONamespace>GAZ</oboInOwl:hasOBONamespace>
        <oboInOwl:id>GAZ:00248013</oboInOwl:id>
        <rdfs:label>Birkat Siwah</rdfs:label>
    </owl:NamedIndividual>
    


    <!-- http://purl.obolibrary.org/obo/GAZ_00248014 -->

    <owl:NamedIndividual rdf:about="http://purl.obolibrary.org/obo/GAZ_00248014">
        <obo:RO_0001025 rdf:resource="http://purl.obolibrary.org/obo/GAZ_00248009"/>
        <obo:IAO_0000115>A saline lake.</obo:IAO_0000115>
        <oboInOwl:hasOBONamespace>GAZ</oboInOwl:hasOBONamespace>
        <oboInOwl:id>GAZ:00248014</oboInOwl:id>
        <rdfs:label>Birkat Aghurmi</rdfs:label>
    </owl:NamedIndividual>
    


    <!-- http://purl.obolibrary.org/obo/GAZ_00248015 -->

    <owl:NamedIndividual rdf:about="http://purl.obolibrary.org/obo/GAZ_00248015">
        <obo:RO_0001025 rdf:resource="http://purl.obolibrary.org/obo/GAZ_00248009"/>
        <obo:IAO_0000115>A saline lake.</obo:IAO_0000115>
        <oboInOwl:hasOBONamespace>GAZ</oboInOwl:hasOBONamespace>
        <oboInOwl:id>GAZ:00248015</oboInOwl:id>
        <rdfs:label>Birkat Samar Abu Ishaq</rdfs:label>
    </owl:NamedIndividual>
    


    <!-- http://purl.obolibrary.org/obo/GAZ_00248016 -->

    <owl:NamedIndividual rdf:about="http://purl.obolibrary.org/obo/GAZ_00248016">
        <obo:RO_0001025 rdf:resource="http://purl.obolibrary.org/obo/GAZ_00051196"/>
        <obo:IAO_0000115>A semi-permanent saline lake.</obo:IAO_0000115>
        <oboInOwl:hasOBONamespace>GAZ</oboInOwl:hasOBONamespace>
        <oboInOwl:id>GAZ:00248016</oboInOwl:id>
        <rdfs:label>Lake Sitra</rdfs:label>
    </owl:NamedIndividual>
    


    <!-- http://purl.obolibrary.org/obo/GAZ_00248017 -->

    <owl:NamedIndividual rdf:about="http://purl.obolibrary.org/obo/GAZ_00248017">
        <obo:RO_0001025 rdf:resource="http://purl.obolibrary.org/obo/GAZ_00051196"/>
        <obo:IAO_0000115>A semi-permanent saline lake.</obo:IAO_0000115>
        <oboInOwl:hasOBONamespace>GAZ</oboInOwl:hasOBONamespace>
        <oboInOwl:id>GAZ:00248017</oboInOwl:id>
        <rdfs:label>Lake el Bahrein</rdfs:label>
    </owl:NamedIndividual>
    


    <!-- http://purl.obolibrary.org/obo/GAZ_00248018 -->

    <owl:NamedIndividual rdf:about="http://purl.obolibrary.org/obo/GAZ_00248018">
        <obo:RO_0001025 rdf:resource="http://purl.obolibrary.org/obo/GAZ_00051196"/>
        <obo:IAO_0000115>A semi-permanent saline lake.</obo:IAO_0000115>
        <oboInOwl:hasOBONamespace>GAZ</oboInOwl:hasOBONamespace>
        <oboInOwl:id>GAZ:00248018</oboInOwl:id>
        <rdfs:label>Lake el Maghra</rdfs:label>
    </owl:NamedIndividual>
    


    <!-- http://purl.obolibrary.org/obo/GAZ_00248111 -->

    <owl:NamedIndividual rdf:about="http://purl.obolibrary.org/obo/GAZ_00248111">
        <obo:RO_0001025 rdf:resource="http://purl.obolibrary.org/obo/GAZ_00002456"/>
        <obo:IAO_0000115>A bay.</obo:IAO_0000115>
        <oboInOwl:hasOBONamespace>GAZ</oboInOwl:hasOBONamespace>
        <oboInOwl:id>GAZ:00248111</oboInOwl:id>
        <rdfs:label>Mersa Mubarec</rdfs:label>
    </owl:NamedIndividual>
    


    <!-- http://purl.obolibrary.org/obo/GAZ_00248112 -->

    <owl:NamedIndividual rdf:about="http://purl.obolibrary.org/obo/GAZ_00248112">
        <obo:RO_0001025 rdf:resource="http://purl.obolibrary.org/obo/GAZ_00002456"/>
        <obo:IAO_0000115>An inlet.</obo:IAO_0000115>
        <oboInOwl:hasOBONamespace>GAZ</oboInOwl:hasOBONamespace>
        <oboInOwl:id>GAZ:00248112</oboInOwl:id>
        <rdfs:label>Mersa Deresa</rdfs:label>
    </owl:NamedIndividual>
    


    <!-- http://purl.obolibrary.org/obo/GAZ_00248117 -->

    <owl:NamedIndividual rdf:about="http://purl.obolibrary.org/obo/GAZ_00248117">
        <obo:RO_0001025 rdf:resource="http://purl.obolibrary.org/obo/GAZ_00002456"/>
        <obo:IAO_0000115>A bay.</obo:IAO_0000115>
        <oboInOwl:hasOBONamespace>GAZ</oboInOwl:hasOBONamespace>
        <oboInOwl:id>GAZ:00248117</oboInOwl:id>
        <rdfs:label>Assab Bahir Selat&apos;e</rdfs:label>
    </owl:NamedIndividual>
    


    <!-- http://purl.obolibrary.org/obo/GAZ_00248118 -->

    <owl:NamedIndividual rdf:about="http://purl.obolibrary.org/obo/GAZ_00248118">
        <obo:RO_0001025 rdf:resource="http://purl.obolibrary.org/obo/GAZ_00002456"/>
        <obo:RO_0001025 rdf:resource="http://purl.obolibrary.org/obo/GAZ_00248117"/>
        <obo:IAO_0000115>An island.</obo:IAO_0000115>
        <oboInOwl:hasOBONamespace>GAZ</oboInOwl:hasOBONamespace>
        <oboInOwl:id>GAZ:00248118</oboInOwl:id>
        <rdfs:label>Fatuma Deset</rdfs:label>
    </owl:NamedIndividual>
    


    <!-- http://purl.obolibrary.org/obo/GAZ_00251838 -->

    <owl:NamedIndividual rdf:about="http://purl.obolibrary.org/obo/GAZ_00251838">
        <obo:IAO_0000115>An erg.</obo:IAO_0000115>
        <oboInOwl:hasOBONamespace>GAZ</oboInOwl:hasOBONamespace>
        <oboInOwl:id>GAZ:00251838</oboInOwl:id>
        <rdfs:label>Idhan Ubari</rdfs:label>
    </owl:NamedIndividual>
    


    <!-- http://purl.obolibrary.org/obo/GAZ_00252194 -->

    <owl:NamedIndividual rdf:about="http://purl.obolibrary.org/obo/GAZ_00252194">
        <obo:RO_0001025 rdf:resource="http://purl.obolibrary.org/obo/GAZ_00252195"/>
        <obo:IAO_0000115>A guelta system.</obo:IAO_0000115>
        <oboInOwl:hasOBONamespace>GAZ</oboInOwl:hasOBONamespace>
        <oboInOwl:id>GAZ:00252194</oboInOwl:id>
        <rdfs:label>Gamra Ouarbi Gueltas</rdfs:label>
    </owl:NamedIndividual>
    


    <!-- http://purl.obolibrary.org/obo/GAZ_00252195 -->

    <owl:NamedIndividual rdf:about="http://purl.obolibrary.org/obo/GAZ_00252195">
        <obo:RO_0001025 rdf:resource="http://purl.obolibrary.org/obo/GAZ_00231580"/>
        <obo:IAO_0000115>A wadi.</obo:IAO_0000115>
        <oboInOwl:hasOBONamespace>GAZ</oboInOwl:hasOBONamespace>
        <oboInOwl:id>GAZ:00252195</oboInOwl:id>
        <rdfs:label>Oued Bourraga</rdfs:label>
    </owl:NamedIndividual>
    


    <!-- http://purl.obolibrary.org/obo/GAZ_00252196 -->

    <owl:NamedIndividual rdf:about="http://purl.obolibrary.org/obo/GAZ_00252196">
        <obo:RO_0001025 rdf:resource="http://purl.obolibrary.org/obo/GAZ_00252195"/>
        <obo:IAO_0000115>A spring.</obo:IAO_0000115>
        <oboInOwl:hasOBONamespace>GAZ</oboInOwl:hasOBONamespace>
        <oboInOwl:id>GAZ:00252196</oboInOwl:id>
        <rdfs:label>El Housseiniya</rdfs:label>
    </owl:NamedIndividual>
    


    <!-- http://purl.obolibrary.org/obo/GAZ_00252197 -->

    <owl:NamedIndividual rdf:about="http://purl.obolibrary.org/obo/GAZ_00252197">
        <obo:RO_0001025 rdf:resource="http://purl.obolibrary.org/obo/GAZ_00231580"/>
        <obo:IAO_0000115>An oasis. Located in the escarpment of the Tagant Plateau, in its southwestern extension towards Kiffa.</obo:IAO_0000115>
        <oboInOwl:hasOBONamespace>GAZ</oboInOwl:hasOBONamespace>
        <oboInOwl:id>GAZ:00252197</oboInOwl:id>
        <rdfs:label>Tartega Gueltas</rdfs:label>
    </owl:NamedIndividual>
    


    <!-- http://purl.obolibrary.org/obo/GAZ_00253017 -->

    <owl:NamedIndividual rdf:about="http://purl.obolibrary.org/obo/GAZ_00253017">
        <obo:RO_0001025 rdf:resource="http://purl.obolibrary.org/obo/GAZ_00103898"/>
        <obo:IAO_0000115>A wadi.</obo:IAO_0000115>
        <oboInOwl:hasOBONamespace>GAZ</oboInOwl:hasOBONamespace>
        <oboInOwl:id>GAZ:00253017</oboInOwl:id>
        <rdfs:label>Ighalabelabene</rdfs:label>
    </owl:NamedIndividual>
    


    <!-- http://purl.obolibrary.org/obo/GAZ_00253018 -->

    <owl:NamedIndividual rdf:about="http://purl.obolibrary.org/obo/GAZ_00253018">
        <obo:RO_0001025 rdf:resource="http://purl.obolibrary.org/obo/GAZ_00103898"/>
        <obo:IAO_0000115>A wadi.</obo:IAO_0000115>
        <oboInOwl:hasOBONamespace>GAZ</oboInOwl:hasOBONamespace>
        <oboInOwl:id>GAZ:00253018</oboInOwl:id>
        <rdfs:label>Nabarou</rdfs:label>
    </owl:NamedIndividual>
    


    <!-- http://purl.obolibrary.org/obo/GAZ_00253019 -->

    <owl:NamedIndividual rdf:about="http://purl.obolibrary.org/obo/GAZ_00253019">
        <obo:RO_0001025 rdf:resource="http://purl.obolibrary.org/obo/GAZ_00103898"/>
        <obo:IAO_0000115>A wadi.</obo:IAO_0000115>
        <oboInOwl:hasOBONamespace>GAZ</oboInOwl:hasOBONamespace>
        <oboInOwl:id>GAZ:00253019</oboInOwl:id>
        <rdfs:label>Bagzane-n-Ammas</rdfs:label>
    </owl:NamedIndividual>
    


    <!-- http://purl.obolibrary.org/obo/GAZ_00253020 -->

    <owl:NamedIndividual rdf:about="http://purl.obolibrary.org/obo/GAZ_00253020">
        <obo:RO_0001025 rdf:resource="http://purl.obolibrary.org/obo/GAZ_00103898"/>
        <obo:IAO_0000115>An intermittent river.</obo:IAO_0000115>
        <oboInOwl:hasOBONamespace>GAZ</oboInOwl:hasOBONamespace>
        <oboInOwl:id>GAZ:00253020</oboInOwl:id>
        <rdfs:label>Timia</rdfs:label>
    </owl:NamedIndividual>
    


    <!-- http://purl.obolibrary.org/obo/GAZ_00253021 -->

    <owl:NamedIndividual rdf:about="http://purl.obolibrary.org/obo/GAZ_00253021">
        <obo:RO_0001025 rdf:resource="http://purl.obolibrary.org/obo/GAZ_00103898"/>
        <obo:IAO_0000115>A wadi.</obo:IAO_0000115>
        <oboInOwl:hasOBONamespace>GAZ</oboInOwl:hasOBONamespace>
        <oboInOwl:id>GAZ:00253021</oboInOwl:id>
        <rdfs:label>Tamgak</rdfs:label>
    </owl:NamedIndividual>
    


    <!-- http://purl.obolibrary.org/obo/GAZ_00253022 -->

    <owl:NamedIndividual rdf:about="http://purl.obolibrary.org/obo/GAZ_00253022">
        <obo:RO_0001025 rdf:resource="http://purl.obolibrary.org/obo/GAZ_00103898"/>
        <obo:IAO_0000115>A plateau.</obo:IAO_0000115>
        <oboInOwl:hasOBONamespace>GAZ</oboInOwl:hasOBONamespace>
        <oboInOwl:id>GAZ:00253022</oboInOwl:id>
        <rdfs:label>Djado Massif</rdfs:label>
    </owl:NamedIndividual>
    


    <!-- http://purl.obolibrary.org/obo/GAZ_00253023 -->

    <owl:NamedIndividual rdf:about="http://purl.obolibrary.org/obo/GAZ_00253023">
        <obo:RO_0001025 rdf:resource="http://purl.obolibrary.org/obo/GAZ_00103898"/>
        <obo:IAO_0000115>A plateau.</obo:IAO_0000115>
        <oboInOwl:hasOBONamespace>GAZ</oboInOwl:hasOBONamespace>
        <oboInOwl:id>GAZ:00253023</oboInOwl:id>
        <rdfs:label>Kaquar Massif</rdfs:label>
    </owl:NamedIndividual>
    


    <!-- http://purl.obolibrary.org/obo/GAZ_00253024 -->

    <owl:NamedIndividual rdf:about="http://purl.obolibrary.org/obo/GAZ_00253024">
        <obo:RO_0001025 rdf:resource="http://purl.obolibrary.org/obo/GAZ_00103898"/>
        <obo:IAO_0000115>An escarpment.</obo:IAO_0000115>
        <oboInOwl:hasOBONamespace>GAZ</oboInOwl:hasOBONamespace>
        <oboInOwl:id>GAZ:00253024</oboInOwl:id>
        <rdfs:label>Fachi Massif</rdfs:label>
    </owl:NamedIndividual>
    


    <!-- http://purl.obolibrary.org/obo/GAZ_00256448 -->

    <owl:NamedIndividual rdf:about="http://purl.obolibrary.org/obo/GAZ_00256448">
        <obo:RO_0001025 rdf:resource="http://purl.obolibrary.org/obo/GAZ_00002456"/>
        <obo:IAO_0000115>A bay.</obo:IAO_0000115>
        <oboInOwl:hasOBONamespace>GAZ</oboInOwl:hasOBONamespace>
        <oboInOwl:id>GAZ:00256448</oboInOwl:id>
        <rdfs:label>Dungunab Bay</rdfs:label>
    </owl:NamedIndividual>
    


    <!-- http://purl.obolibrary.org/obo/GAZ_00256449 -->

    <owl:NamedIndividual rdf:about="http://purl.obolibrary.org/obo/GAZ_00256449">
        <obo:RO_0001025 rdf:resource="http://purl.obolibrary.org/obo/GAZ_00000685"/>
        <obo:RO_0001025 rdf:resource="http://purl.obolibrary.org/obo/GAZ_00002456"/>
        <obo:IAO_0000115>An island.</obo:IAO_0000115>
        <oboInOwl:hasOBONamespace>GAZ</oboInOwl:hasOBONamespace>
        <oboInOwl:id>GAZ:00256449</oboInOwl:id>
        <rdfs:label>Jazirat Mukawwa&apos;</rdfs:label>
    </owl:NamedIndividual>
    


    <!-- http://purl.obolibrary.org/obo/GAZ_00256450 -->

    <owl:NamedIndividual rdf:about="http://purl.obolibrary.org/obo/GAZ_00256450">
        <obo:RO_0001025 rdf:resource="http://purl.obolibrary.org/obo/GAZ_00000685"/>
        <obo:IAO_0000115>A bay.</obo:IAO_0000115>
        <oboInOwl:hasOBONamespace>GAZ</oboInOwl:hasOBONamespace>
        <oboInOwl:id>GAZ:00256450</oboInOwl:id>
        <rdfs:label>Gulf of Aqiq</rdfs:label>
    </owl:NamedIndividual>
    


    <!-- http://purl.obolibrary.org/obo/GAZ_00256465 -->

    <owl:NamedIndividual rdf:about="http://purl.obolibrary.org/obo/GAZ_00256465">
        <obo:IAO_0000115>A river.</obo:IAO_0000115>
        <oboInOwl:hasOBONamespace>GAZ</oboInOwl:hasOBONamespace>
        <oboInOwl:id>GAZ:00256465</oboInOwl:id>
        <rdfs:label>Lileboak River</rdfs:label>
    </owl:NamedIndividual>
    


    <!-- http://purl.obolibrary.org/obo/GAZ_00256471 -->

    <owl:NamedIndividual rdf:about="http://purl.obolibrary.org/obo/GAZ_00256471">
        <obo:RO_0001025 rdf:resource="http://purl.obolibrary.org/obo/GAZ_00076687"/>
        <obo:IAO_0000115>A floodplain that occupies the land between the Dinder and Rahad Rivers which flow down from the Ethiopian Highlands to a flat plain, sloping gently northwestwards towards the Blue Nile.</obo:IAO_0000115>
        <oboInOwl:hasOBONamespace>GAZ</oboInOwl:hasOBONamespace>
        <oboInOwl:id>GAZ:00256471</oboInOwl:id>
        <rdfs:label>Dinder Floodplain</rdfs:label>
    </owl:NamedIndividual>
    


    <!-- http://purl.obolibrary.org/obo/GAZ_00256472 -->

    <owl:NamedIndividual rdf:about="http://purl.obolibrary.org/obo/GAZ_00256472">
        <obo:RO_0001025 rdf:resource="http://purl.obolibrary.org/obo/GAZ_00000679"/>
        <obo:IAO_0000115>A dam.</obo:IAO_0000115>
        <oboInOwl:hasOBONamespace>GAZ</oboInOwl:hasOBONamespace>
        <oboInOwl:id>GAZ:00256472</oboInOwl:id>
        <rdfs:label>Jebel Auliya Dam</rdfs:label>
    </owl:NamedIndividual>
    


    <!-- http://purl.obolibrary.org/obo/GAZ_00256473 -->

    <owl:NamedIndividual rdf:about="http://purl.obolibrary.org/obo/GAZ_00256473">
        <obo:RO_0001025 rdf:resource="http://purl.obolibrary.org/obo/GAZ_00000679"/>
        <obo:IAO_0000115>A reservoir. Impounded by Jebel Auliya Dam.</obo:IAO_0000115>
        <oboInOwl:hasOBONamespace>GAZ</oboInOwl:hasOBONamespace>
        <oboInOwl:id>GAZ:00256473</oboInOwl:id>
        <rdfs:label>Jebel Auliya Reservoir</rdfs:label>
    </owl:NamedIndividual>
    


    <!-- http://purl.obolibrary.org/obo/GAZ_00256474 -->

    <owl:NamedIndividual rdf:about="http://purl.obolibrary.org/obo/GAZ_00256474">
        <obo:RO_0001025 rdf:resource="http://purl.obolibrary.org/obo/GAZ_00000683"/>
        <obo:IAO_0000115>An endorheic lake situated on the plateau of Kurdufan.</obo:IAO_0000115>
        <oboInOwl:hasOBONamespace>GAZ</oboInOwl:hasOBONamespace>
        <oboInOwl:id>GAZ:00256474</oboInOwl:id>
        <rdfs:label>Lake Keilack</rdfs:label>
    </owl:NamedIndividual>
    


    <!-- http://purl.obolibrary.org/obo/GAZ_00256475 -->

    <owl:NamedIndividual rdf:about="http://purl.obolibrary.org/obo/GAZ_00256475">
        <obo:RO_0001025 rdf:resource="http://purl.obolibrary.org/obo/GAZ_00000688"/>
        <obo:IAO_0000115>An endorheic lake.</obo:IAO_0000115>
        <oboInOwl:hasOBONamespace>GAZ</oboInOwl:hasOBONamespace>
        <oboInOwl:id>GAZ:00256475</oboInOwl:id>
        <rdfs:label>Lake Kundi</rdfs:label>
    </owl:NamedIndividual>
    


    <!-- http://purl.obolibrary.org/obo/GAZ_00256482 -->

    <owl:NamedIndividual rdf:about="http://purl.obolibrary.org/obo/GAZ_00256482">
        <obo:RO_0001025 rdf:resource="http://purl.obolibrary.org/obo/GAZ_00000674"/>
        <obo:IAO_0000115>An artificial lake. Impounded by El Roseires Dam.</obo:IAO_0000115>
        <oboInOwl:hasOBONamespace>GAZ</oboInOwl:hasOBONamespace>
        <oboInOwl:id>GAZ:00256482</oboInOwl:id>
        <rdfs:label>El Roseires Lake</rdfs:label>
    </owl:NamedIndividual>
    


    <!-- http://purl.obolibrary.org/obo/GAZ_00256483 -->

    <owl:NamedIndividual rdf:about="http://purl.obolibrary.org/obo/GAZ_00256483">
        <obo:RO_0001025 rdf:resource="http://purl.obolibrary.org/obo/GAZ_00000687"/>
        <obo:IAO_0000115>An artifiical lake. Impounded by Sennar Dam.</obo:IAO_0000115>
        <oboInOwl:hasOBONamespace>GAZ</oboInOwl:hasOBONamespace>
        <oboInOwl:id>GAZ:00256483</oboInOwl:id>
        <rdfs:label>Sennar Lake</rdfs:label>
    </owl:NamedIndividual>
    


    <!-- http://purl.obolibrary.org/obo/GAZ_00256484 -->

    <owl:NamedIndividual rdf:about="http://purl.obolibrary.org/obo/GAZ_00256484">
        <obo:IAO_0000115>A dam. Impounds Kashim el Girlba Lake. Completed 1964.</obo:IAO_0000115>
        <oboInOwl:hasOBONamespace>GAZ</oboInOwl:hasOBONamespace>
        <oboInOwl:id>GAZ:00256484</oboInOwl:id>
        <rdfs:label>Kashim el Girlba Dam</rdfs:label>
    </owl:NamedIndividual>
    


    <!-- http://purl.obolibrary.org/obo/GAZ_00256485 -->

    <owl:NamedIndividual rdf:about="http://purl.obolibrary.org/obo/GAZ_00256485">
        <obo:IAO_0000115>An artifiical lake. Impounded by Kashim el Girlba Dam. Completed 1964.</obo:IAO_0000115>
        <oboInOwl:hasOBONamespace>GAZ</oboInOwl:hasOBONamespace>
        <oboInOwl:id>GAZ:00256485</oboInOwl:id>
        <rdfs:label>Kashim el Girlba Lake</rdfs:label>
    </owl:NamedIndividual>
    


    <!-- http://purl.obolibrary.org/obo/GAZ_00256486 -->

    <owl:NamedIndividual rdf:about="http://purl.obolibrary.org/obo/GAZ_00256486">
        <rdf:type rdf:resource="http://purl.obolibrary.org/obo/ENVO_00000074"/>
        <obo:RO_0001025 rdf:resource="http://purl.obolibrary.org/obo/GAZ_00000679"/>
        <obo:IAO_0000115>A barrage. Located 25 km S of Khartoum.</obo:IAO_0000115>
        <oboInOwl:hasOBONamespace>GAZ</oboInOwl:hasOBONamespace>
        <oboInOwl:id>GAZ:00256486</oboInOwl:id>
        <rdfs:label>Gebel Auliya</rdfs:label>
    </owl:NamedIndividual>
    


    <!-- http://purl.obolibrary.org/obo/GAZ_00260292 -->

    <owl:NamedIndividual rdf:about="http://purl.obolibrary.org/obo/GAZ_00260292">
        <rdf:type rdf:resource="http://purl.obolibrary.org/obo/ENVO_00000475"/>
        <obo:RO_0001025 rdf:resource="http://purl.obolibrary.org/obo/GAZ_00058791"/>
        <obo:IAO_0000115>An arm of Lake Kyoga.</obo:IAO_0000115>
        <oboInOwl:hasOBONamespace>GAZ</oboInOwl:hasOBONamespace>
        <oboInOwl:id>GAZ:00260292</oboInOwl:id>
        <rdfs:label>Mpologoma Arm</rdfs:label>
    </owl:NamedIndividual>
    


    <!-- http://purl.obolibrary.org/obo/GAZ_00260861 -->

    <owl:NamedIndividual rdf:about="http://purl.obolibrary.org/obo/GAZ_00260861">
        <obo:RO_0001025 rdf:resource="http://purl.obolibrary.org/obo/GAZ_00002456"/>
        <obo:IAO_0000115>An island.</obo:IAO_0000115>
        <oboInOwl:hasOBONamespace>GAZ</oboInOwl:hasOBONamespace>
        <oboInOwl:id>GAZ:00260861</oboInOwl:id>
        <rdfs:label>Buhays Island</rdfs:label>
    </owl:NamedIndividual>
    


    <!-- http://purl.obolibrary.org/obo/GAZ_00260862 -->

    <owl:NamedIndividual rdf:about="http://purl.obolibrary.org/obo/GAZ_00260862">
        <obo:RO_0001025 rdf:resource="http://purl.obolibrary.org/obo/GAZ_00002456"/>
        <oboInOwl:hasOBONamespace>GAZ</oboInOwl:hasOBONamespace>
        <oboInOwl:id>GAZ:00260862</oboInOwl:id>
        <rdfs:label>Al-Badi Island</rdfs:label>
    </owl:NamedIndividual>
    


    <!-- http://purl.obolibrary.org/obo/GAZ_00260863 -->

    <owl:NamedIndividual rdf:about="http://purl.obolibrary.org/obo/GAZ_00260863">
        <obo:RO_0001025 rdf:resource="http://purl.obolibrary.org/obo/GAZ_00002456"/>
        <obo:IAO_0000115>An island.</obo:IAO_0000115>
        <oboInOwl:hasOBONamespace>GAZ</oboInOwl:hasOBONamespace>
        <oboInOwl:id>GAZ:00260863</oboInOwl:id>
        <rdfs:label>Tikfash Island</rdfs:label>
    </owl:NamedIndividual>
    


    <!-- http://purl.obolibrary.org/obo/GAZ_00260864 -->

    <owl:NamedIndividual rdf:about="http://purl.obolibrary.org/obo/GAZ_00260864">
        <obo:RO_0001025 rdf:resource="http://purl.obolibrary.org/obo/GAZ_00002456"/>
        <obo:IAO_0000115>An island.</obo:IAO_0000115>
        <oboInOwl:hasOBONamespace>GAZ</oboInOwl:hasOBONamespace>
        <oboInOwl:id>GAZ:00260864</oboInOwl:id>
        <rdfs:label>Humar Island</rdfs:label>
    </owl:NamedIndividual>
    


    <!-- http://purl.obolibrary.org/obo/GAZ_00260865 -->

    <owl:NamedIndividual rdf:about="http://purl.obolibrary.org/obo/GAZ_00260865">
        <obo:RO_0001025 rdf:resource="http://purl.obolibrary.org/obo/GAZ_00002456"/>
        <obo:IAO_0000115>An island.</obo:IAO_0000115>
        <oboInOwl:hasOBONamespace>GAZ</oboInOwl:hasOBONamespace>
        <oboInOwl:id>GAZ:00260865</oboInOwl:id>
        <rdfs:label>Kitamah Island</rdfs:label>
    </owl:NamedIndividual>
    


    <!-- http://purl.obolibrary.org/obo/GAZ_00260866 -->

    <owl:NamedIndividual rdf:about="http://purl.obolibrary.org/obo/GAZ_00260866">
        <obo:RO_0001025 rdf:resource="http://purl.obolibrary.org/obo/GAZ_00002456"/>
        <obo:IAO_0000115>An island.</obo:IAO_0000115>
        <oboInOwl:hasOBONamespace>GAZ</oboInOwl:hasOBONamespace>
        <oboInOwl:id>GAZ:00260866</oboInOwl:id>
        <rdfs:label>Zakhah Island</rdfs:label>
    </owl:NamedIndividual>
    


    <!-- http://purl.obolibrary.org/obo/GAZ_00260867 -->

    <owl:NamedIndividual rdf:about="http://purl.obolibrary.org/obo/GAZ_00260867">
        <obo:RO_0001025 rdf:resource="http://purl.obolibrary.org/obo/GAZ_00002456"/>
        <obo:IAO_0000115>An island.</obo:IAO_0000115>
        <oboInOwl:hasOBONamespace>GAZ</oboInOwl:hasOBONamespace>
        <oboInOwl:id>GAZ:00260867</oboInOwl:id>
        <rdfs:label>Zurbat Island</rdfs:label>
    </owl:NamedIndividual>
    


    <!-- http://purl.obolibrary.org/obo/GAZ_00260868 -->

    <owl:NamedIndividual rdf:about="http://purl.obolibrary.org/obo/GAZ_00260868">
        <obo:RO_0001025 rdf:resource="http://purl.obolibrary.org/obo/GAZ_00002456"/>
        <obo:IAO_0000115>An island.</obo:IAO_0000115>
        <oboInOwl:hasOBONamespace>GAZ</oboInOwl:hasOBONamespace>
        <oboInOwl:id>GAZ:00260868</oboInOwl:id>
        <rdfs:label>Juwa Island</rdfs:label>
    </owl:NamedIndividual>
    


    <!-- http://purl.obolibrary.org/obo/GAZ_00260869 -->

    <owl:NamedIndividual rdf:about="http://purl.obolibrary.org/obo/GAZ_00260869">
        <obo:RO_0001025 rdf:resource="http://purl.obolibrary.org/obo/GAZ_00002456"/>
        <obo:IAO_0000115>An island.</obo:IAO_0000115>
        <oboInOwl:hasOBONamespace>GAZ</oboInOwl:hasOBONamespace>
        <oboInOwl:id>GAZ:00260869</oboInOwl:id>
        <rdfs:label>At Talawin Island</rdfs:label>
    </owl:NamedIndividual>
    


    <!-- http://purl.obolibrary.org/obo/GAZ_00260871 -->

    <owl:NamedIndividual rdf:about="http://purl.obolibrary.org/obo/GAZ_00260871">
        <obo:RO_0001025 rdf:resource="http://purl.obolibrary.org/obo/GAZ_00002456"/>
        <obo:IAO_0000115>An island.</obo:IAO_0000115>
        <oboInOwl:hasOBONamespace>GAZ</oboInOwl:hasOBONamespace>
        <oboInOwl:id>GAZ:00260871</oboInOwl:id>
        <rdfs:label>Zabin Island</rdfs:label>
    </owl:NamedIndividual>
    


    <!-- http://purl.obolibrary.org/obo/GAZ_00260872 -->

    <owl:NamedIndividual rdf:about="http://purl.obolibrary.org/obo/GAZ_00260872">
        <obo:RO_0001025 rdf:resource="http://purl.obolibrary.org/obo/GAZ_00002456"/>
        <obo:IAO_0000115>An island.</obo:IAO_0000115>
        <oboInOwl:hasOBONamespace>GAZ</oboInOwl:hasOBONamespace>
        <oboInOwl:id>GAZ:00260872</oboInOwl:id>
        <rdfs:label>Al-Murk Island</rdfs:label>
    </owl:NamedIndividual>
    


    <!-- http://purl.obolibrary.org/obo/GAZ_00260873 -->

    <owl:NamedIndividual rdf:about="http://purl.obolibrary.org/obo/GAZ_00260873">
        <obo:RO_0001025 rdf:resource="http://purl.obolibrary.org/obo/GAZ_00002456"/>
        <obo:IAO_0000115>An island.</obo:IAO_0000115>
        <oboInOwl:hasOBONamespace>GAZ</oboInOwl:hasOBONamespace>
        <oboInOwl:id>GAZ:00260873</oboInOwl:id>
        <rdfs:label>Hataban Island</rdfs:label>
    </owl:NamedIndividual>
    


    <!-- http://purl.obolibrary.org/obo/GAZ_00260874 -->

    <owl:NamedIndividual rdf:about="http://purl.obolibrary.org/obo/GAZ_00260874">
        <obo:RO_0001025 rdf:resource="http://purl.obolibrary.org/obo/GAZ_00002456"/>
        <obo:IAO_0000115>An island.</obo:IAO_0000115>
        <oboInOwl:hasOBONamespace>GAZ</oboInOwl:hasOBONamespace>
        <oboInOwl:id>GAZ:00260874</oboInOwl:id>
        <rdfs:label>&apos;Ukban Island</rdfs:label>
    </owl:NamedIndividual>
    


    <!-- http://purl.obolibrary.org/obo/GAZ_00260875 -->

    <owl:NamedIndividual rdf:about="http://purl.obolibrary.org/obo/GAZ_00260875">
        <obo:RO_0001025 rdf:resource="http://purl.obolibrary.org/obo/GAZ_00002456"/>
        <obo:IAO_0000115>An island.</obo:IAO_0000115>
        <oboInOwl:hasOBONamespace>GAZ</oboInOwl:hasOBONamespace>
        <oboInOwl:id>GAZ:00260875</oboInOwl:id>
        <rdfs:label>Bahr Ibn Abbas</rdfs:label>
    </owl:NamedIndividual>
    


    <!-- http://purl.obolibrary.org/obo/GAZ_00281380 -->

    <owl:NamedIndividual rdf:about="http://purl.obolibrary.org/obo/GAZ_00281380">
        <obo:RO_0001025 rdf:resource="http://purl.obolibrary.org/obo/GAZ_00000686"/>
        <obo:IAO_0000115>An island.</obo:IAO_0000115>
        <oboInOwl:hasOBONamespace>GAZ</oboInOwl:hasOBONamespace>
        <oboInOwl:id>GAZ:00281380</oboInOwl:id>
        <rdfs:label>Us Island</rdfs:label>
    </owl:NamedIndividual>
    


    <!-- http://purl.obolibrary.org/obo/GAZ_00281381 -->

    <owl:NamedIndividual rdf:about="http://purl.obolibrary.org/obo/GAZ_00281381">
        <obo:RO_0001025 rdf:resource="http://purl.obolibrary.org/obo/GAZ_00000686"/>
        <obo:IAO_0000115>An island.</obo:IAO_0000115>
        <oboInOwl:hasOBONamespace>GAZ</oboInOwl:hasOBONamespace>
        <oboInOwl:id>GAZ:00281381</oboInOwl:id>
        <rdfs:label>Sur Island</rdfs:label>
    </owl:NamedIndividual>
    


    <!-- http://purl.obolibrary.org/obo/GAZ_00281382 -->

    <owl:NamedIndividual rdf:about="http://purl.obolibrary.org/obo/GAZ_00281382">
        <obo:RO_0001025 rdf:resource="http://purl.obolibrary.org/obo/GAZ_00000686"/>
        <obo:IAO_0000115>An island.</obo:IAO_0000115>
        <oboInOwl:hasOBONamespace>GAZ</oboInOwl:hasOBONamespace>
        <oboInOwl:id>GAZ:00281382</oboInOwl:id>
        <rdfs:label>Sherari Island</rdfs:label>
    </owl:NamedIndividual>
    


    <!-- http://purl.obolibrary.org/obo/GAZ_00281383 -->

    <owl:NamedIndividual rdf:about="http://purl.obolibrary.org/obo/GAZ_00281383">
        <obo:RO_0001025 rdf:resource="http://purl.obolibrary.org/obo/GAZ_00000684"/>
        <obo:IAO_0000115>A populated place.</obo:IAO_0000115>
        <oboInOwl:hasOBONamespace>GAZ</oboInOwl:hasOBONamespace>
        <oboInOwl:id>GAZ:00281383</oboInOwl:id>
        <rdfs:label>Karima</rdfs:label>
    </owl:NamedIndividual>
    


    <!-- http://purl.obolibrary.org/obo/GAZ_00281384 -->

    <owl:NamedIndividual rdf:about="http://purl.obolibrary.org/obo/GAZ_00281384">
        <obo:RO_0001025 rdf:resource="http://purl.obolibrary.org/obo/GAZ_00281383"/>
        <obo:IAO_0000115>A small mountain located some 400 km north of Khartoum, in Karima town in Northern State in Sudan, on a large bend of the Nile River.</obo:IAO_0000115>
        <oboInOwl:hasOBONamespace>GAZ</oboInOwl:hasOBONamespace>
        <oboInOwl:id>GAZ:00281384</oboInOwl:id>
        <rdfs:label>Jebel Barkal</rdfs:label>
    </owl:NamedIndividual>
    


    <!-- http://purl.obolibrary.org/obo/GAZ_00281385 -->

    <owl:NamedIndividual rdf:about="http://purl.obolibrary.org/obo/GAZ_00281385">
        <obo:RO_0001025 rdf:resource="http://purl.obolibrary.org/obo/GAZ_00281383"/>
        <obo:IAO_0000115>An archeological site on, and in the vicinity of Jebel barkal.</obo:IAO_0000115>
        <oboInOwl:hasOBONamespace>GAZ</oboInOwl:hasOBONamespace>
        <oboInOwl:id>GAZ:00281385</oboInOwl:id>
        <rdfs:label>Jebel Barkal [site]</rdfs:label>
    </owl:NamedIndividual>
    


    <!-- http://purl.obolibrary.org/obo/GAZ_00281386 -->

    <owl:NamedIndividual rdf:about="http://purl.obolibrary.org/obo/GAZ_00281386">
        <obo:RO_0001025 rdf:resource="http://purl.obolibrary.org/obo/GAZ_00032273"/>
        <obo:IAO_0000115>An archeological site. It was the capital of the Kingdom of Kush. It is marked by more than two hundred pyramids in three groups.</obo:IAO_0000115>
        <oboInOwl:hasOBONamespace>GAZ</oboInOwl:hasOBONamespace>
        <oboInOwl:id>GAZ:00281386</oboInOwl:id>
        <rdfs:label>Meroe</rdfs:label>
    </owl:NamedIndividual>
    


    <!-- http://purl.obolibrary.org/obo/GAZ_00281387 -->

    <owl:NamedIndividual rdf:about="http://purl.obolibrary.org/obo/GAZ_00281387">
        <obo:RO_0001025 rdf:resource="http://purl.obolibrary.org/obo/GAZ_00000686"/>
        <obo:IAO_0000115>An archeological site. A ruined ancient city of the Kushitic Kingdom of Meroe.</obo:IAO_0000115>
        <oboInOwl:hasOBONamespace>GAZ</oboInOwl:hasOBONamespace>
        <oboInOwl:id>GAZ:00281387</oboInOwl:id>
        <rdfs:label>Naqa</rdfs:label>
    </owl:NamedIndividual>
    


    <!-- http://purl.obolibrary.org/obo/GAZ_00281388 -->

    <owl:NamedIndividual rdf:about="http://purl.obolibrary.org/obo/GAZ_00281388">
        <obo:RO_0001025 rdf:resource="http://purl.obolibrary.org/obo/GAZ_00000686"/>
        <obo:IAO_0000115>An archeological site. An ancient town of the Kushitic Kingdom of Meroe.</obo:IAO_0000115>
        <oboInOwl:hasOBONamespace>GAZ</oboInOwl:hasOBONamespace>
        <oboInOwl:id>GAZ:00281388</oboInOwl:id>
        <rdfs:label>Wad ban Naqa</rdfs:label>
    </owl:NamedIndividual>
    


    <!-- http://purl.obolibrary.org/obo/GAZ_00281389 -->

    <owl:NamedIndividual rdf:about="http://purl.obolibrary.org/obo/GAZ_00281389">
        <obo:RO_0001025 rdf:resource="http://purl.obolibrary.org/obo/GAZ_00000684"/>
        <obo:IAO_0000115>An archeological site. The location of a fortified town established in the reign of Senusret I (1965-1920 BC) on the west bank of the Nile at the southern end of a series of fortresses founded during the 12th Dynasty (1985-1795 BC) in the second-cataract area of Lower Nubia.</obo:IAO_0000115>
        <oboInOwl:hasOBONamespace>GAZ</oboInOwl:hasOBONamespace>
        <oboInOwl:id>GAZ:00281389</oboInOwl:id>
        <rdfs:label>Semna</rdfs:label>
    </owl:NamedIndividual>
    


    <!-- http://purl.obolibrary.org/obo/GAZ_00281390 -->

    <owl:NamedIndividual rdf:about="http://purl.obolibrary.org/obo/GAZ_00281390">
        <obo:RO_0001025 rdf:resource="http://purl.obolibrary.org/obo/GAZ_00000684"/>
        <obo:IAO_0000115>An archeological site. An ancient Egyptian settlement located on an island in the Nile above (to the South of) the Second Cataract.</obo:IAO_0000115>
        <oboInOwl:hasOBONamespace>GAZ</oboInOwl:hasOBONamespace>
        <oboInOwl:id>GAZ:00281390</oboInOwl:id>
        <rdfs:label>Uronarti</rdfs:label>
    </owl:NamedIndividual>
    


    <!-- http://purl.obolibrary.org/obo/GAZ_00281422 -->

    <owl:NamedIndividual rdf:about="http://purl.obolibrary.org/obo/GAZ_00281422">
        <obo:IAO_0000115>A region in Libya known for extensive prehistoric rock art.</obo:IAO_0000115>
        <oboInOwl:hasOBONamespace>GAZ</oboInOwl:hasOBONamespace>
        <oboInOwl:id>GAZ:00281422</oboInOwl:id>
        <rdfs:label>Mesak Settafet</rdfs:label>
    </owl:NamedIndividual>
    


    <!-- http://purl.obolibrary.org/obo/GAZ_00281423 -->

    <owl:NamedIndividual rdf:about="http://purl.obolibrary.org/obo/GAZ_00281423">
        <obo:RO_0001025 rdf:resource="http://purl.obolibrary.org/obo/GAZ_00281422"/>
        <obo:IAO_0000115>A prehistoric archeological site in south western Libya in Mesak Settafet, famous for its rock engravings of different kinds.</obo:IAO_0000115>
        <oboInOwl:hasOBONamespace>GAZ</oboInOwl:hasOBONamespace>
        <oboInOwl:id>GAZ:00281423</oboInOwl:id>
        <rdfs:label>Wadi Mathendous</rdfs:label>
    </owl:NamedIndividual>
    


    <!-- http://purl.obolibrary.org/obo/GAZ_00281424 -->

    <owl:NamedIndividual rdf:about="http://purl.obolibrary.org/obo/GAZ_00281424">
        <obo:RO_0001025 rdf:resource="http://purl.obolibrary.org/obo/GAZ_00281422"/>
        <obo:IAO_0000115>A site of rock art.</obo:IAO_0000115>
        <oboInOwl:hasOBONamespace>GAZ</oboInOwl:hasOBONamespace>
        <oboInOwl:id>GAZ:00281424</oboInOwl:id>
        <rdfs:label>Ghalgiwan</rdfs:label>
    </owl:NamedIndividual>
    


    <!-- http://purl.obolibrary.org/obo/GAZ_00281425 -->

    <owl:NamedIndividual rdf:about="http://purl.obolibrary.org/obo/GAZ_00281425">
        <obo:RO_0001025 rdf:resource="http://purl.obolibrary.org/obo/GAZ_00281422"/>
        <obo:IAO_0000115>A site of rock art.</obo:IAO_0000115>
        <oboInOwl:hasOBONamespace>GAZ</oboInOwl:hasOBONamespace>
        <oboInOwl:id>GAZ:00281425</oboInOwl:id>
        <rdfs:label>Tiksaten</rdfs:label>
    </owl:NamedIndividual>
    


    <!-- http://purl.obolibrary.org/obo/GAZ_00281426 -->

    <owl:NamedIndividual rdf:about="http://purl.obolibrary.org/obo/GAZ_00281426">
        <obo:RO_0001025 rdf:resource="http://purl.obolibrary.org/obo/GAZ_00281422"/>
        <obo:IAO_0000115>A site of rock art.</obo:IAO_0000115>
        <oboInOwl:hasOBONamespace>GAZ</oboInOwl:hasOBONamespace>
        <oboInOwl:id>GAZ:00281426</oboInOwl:id>
        <rdfs:label>Abategh</rdfs:label>
    </owl:NamedIndividual>
    


    <!-- http://purl.obolibrary.org/obo/GAZ_00507741 -->

    <owl:NamedIndividual rdf:about="http://purl.obolibrary.org/obo/GAZ_00507741">
        <rdf:type rdf:resource="http://purl.obolibrary.org/obo/ENVO_00000009"/>
        <obo:RO_0001025 rdf:resource="http://purl.obolibrary.org/obo/GAZ_00004036"/>
        <obo:IAO_0000115>A state of Darfur; created 2012-1. The state was formed from land that was previously part of the state of South Darfur.</obo:IAO_0000115>
        <oboInOwl:hasOBONamespace>GAZ</oboInOwl:hasOBONamespace>
        <oboInOwl:id>GAZ:00507741</oboInOwl:id>
        <rdfs:label>East Darfur</rdfs:label>
    </owl:NamedIndividual>
    


    <!-- http://purl.obolibrary.org/obo/GAZ_00507742 -->

    <owl:NamedIndividual rdf:about="http://purl.obolibrary.org/obo/GAZ_00507742">
        <rdf:type rdf:resource="http://purl.obolibrary.org/obo/ENVO_00000009"/>
        <obo:RO_0001025 rdf:resource="http://purl.obolibrary.org/obo/GAZ_00004036"/>
        <obo:IAO_0000115>A state; created 2012-01. The state was formed from land that was previously part of the states of West Darfur and South Darfur.</obo:IAO_0000115>
        <oboInOwl:hasOBONamespace>GAZ</oboInOwl:hasOBONamespace>
        <oboInOwl:id>GAZ:00507742</oboInOwl:id>
        <rdfs:label>Central Darfur</rdfs:label>
    </owl:NamedIndividual>
    


    <!-- http://purl.obolibrary.org/obo/GAZ_00507743 -->

    <owl:NamedIndividual rdf:about="http://purl.obolibrary.org/obo/GAZ_00507743">
        <obo:RO_0001025 rdf:resource="http://purl.obolibrary.org/obo/GAZ_00507741"/>
        <obo:IAO_0000115>A populated place.</obo:IAO_0000115>
        <oboInOwl:hasOBONamespace>GAZ</oboInOwl:hasOBONamespace>
        <oboInOwl:id>GAZ:00507743</oboInOwl:id>
        <rdfs:label>Ed Daein</rdfs:label>
    </owl:NamedIndividual>
    


    <!-- http://purl.obolibrary.org/obo/GAZ_00507744 -->

    <owl:NamedIndividual rdf:about="http://purl.obolibrary.org/obo/GAZ_00507744">
        <rdf:type rdf:resource="http://purl.obolibrary.org/obo/ENVO_00000856"/>
        <obo:RO_0001025 rdf:resource="http://purl.obolibrary.org/obo/GAZ_00032225"/>
        <obo:IAO_0000115>A populated place. A town.</obo:IAO_0000115>
        <oboInOwl:hasOBONamespace>GAZ</oboInOwl:hasOBONamespace>
        <oboInOwl:id>GAZ:00507744</oboInOwl:id>
        <rdfs:label>Abyei Town</rdfs:label>
    </owl:NamedIndividual>
    


    <!-- http://purl.obolibrary.org/obo/GAZ_00507745 -->

    <owl:NamedIndividual rdf:about="http://purl.obolibrary.org/obo/GAZ_00507745">
        <rdf:type rdf:resource="http://purl.obolibrary.org/obo/ENVO_00000856"/>
        <obo:RO_0001025 rdf:resource="http://purl.obolibrary.org/obo/GAZ_00507742"/>
        <obo:IAO_0000115>A populated place. A town.</obo:IAO_0000115>
        <oboInOwl:hasOBONamespace>GAZ</oboInOwl:hasOBONamespace>
        <oboInOwl:id>GAZ:00507745</oboInOwl:id>
        <rdfs:label>Zalingei</rdfs:label>
    </owl:NamedIndividual>
    


    <!-- http://purl.obolibrary.org/obo/GAZ_00507746 -->

    <owl:NamedIndividual rdf:about="http://purl.obolibrary.org/obo/GAZ_00507746">
        <obo:RO_0001025 rdf:resource="http://purl.obolibrary.org/obo/GAZ_00507742"/>
        <obo:IAO_0000115>A refugee camp.</obo:IAO_0000115>
        <oboInOwl:hasOBONamespace>GAZ</oboInOwl:hasOBONamespace>
        <oboInOwl:id>GAZ:00507746</oboInOwl:id>
        <rdfs:label>Hassahissa Internally Displaced Person (IDP) Camp</rdfs:label>
    </owl:NamedIndividual>
    


    <!-- http://purl.obolibrary.org/obo/GAZ_00507747 -->

    <owl:NamedIndividual rdf:about="http://purl.obolibrary.org/obo/GAZ_00507747">
        <obo:RO_0001025 rdf:resource="http://purl.obolibrary.org/obo/GAZ_00507742"/>
        <obo:IAO_0000115>A refugee camp.</obo:IAO_0000115>
        <oboInOwl:hasOBONamespace>GAZ</oboInOwl:hasOBONamespace>
        <oboInOwl:id>GAZ:00507747</oboInOwl:id>
        <rdfs:label>Khamsa Dagayeg Internally Displaced Person (IDP)</rdfs:label>
    </owl:NamedIndividual>
    


    <!-- http://purl.obolibrary.org/obo/GAZ_00507748 -->

    <owl:NamedIndividual rdf:about="http://purl.obolibrary.org/obo/GAZ_00507748">
        <obo:RO_0001025 rdf:resource="http://purl.obolibrary.org/obo/GAZ_00507742"/>
        <obo:IAO_0000115>A refugee camp.</obo:IAO_0000115>
        <oboInOwl:hasOBONamespace>GAZ</oboInOwl:hasOBONamespace>
        <oboInOwl:id>GAZ:00507748</oboInOwl:id>
        <rdfs:label>Hamediya Internally Displaced Person (IDP)</rdfs:label>
    </owl:NamedIndividual>
    


    <!-- http://purl.obolibrary.org/obo/GAZ_00507749 -->

    <owl:NamedIndividual rdf:about="http://purl.obolibrary.org/obo/GAZ_00507749">
        <obo:RO_0001025 rdf:resource="http://purl.obolibrary.org/obo/GAZ_00507742"/>
        <obo:IAO_0000115>A refugee camp.</obo:IAO_0000115>
        <oboInOwl:hasOBONamespace>GAZ</oboInOwl:hasOBONamespace>
        <oboInOwl:id>GAZ:00507749</oboInOwl:id>
        <rdfs:label>Alsalam Internally Displaced Person (IDP)</rdfs:label>
    </owl:NamedIndividual>
    


    <!-- 
    ///////////////////////////////////////////////////////////////////////////////////////
    //
    // Annotations
    //
    ///////////////////////////////////////////////////////////////////////////////////////
     -->

    <rdf:Description rdf:about="http://purl.obolibrary.org/obo/GAZ_00007859">
        <oboInOwl:hasOBONamespace>GAZ</oboInOwl:hasOBONamespace>
        <rdfs:label>populated place, Sudan</rdfs:label>
        <oboInOwl:id>GAZ:00007859</oboInOwl:id>
    </rdf:Description>
    <rdf:Description rdf:about="http://purl.obolibrary.org/obo/GAZ_00007860">
        <rdfs:label>Kosti</rdfs:label>
        <oboInOwl:id>GAZ:00007860</oboInOwl:id>
        <oboInOwl:hasOBONamespace>GAZ</oboInOwl:hasOBONamespace>
    </rdf:Description>
    <rdf:Description rdf:about="http://purl.obolibrary.org/obo/GAZ_00058884">
        <oboInOwl:id>GAZ:00058884</oboInOwl:id>
        <obo:IAO_0000115>Shallow stretches between Aswan and Khartoum where the water&apos;s surface is broken by numerous small boulders and stones lying on the river bed, as well as many small rocky islets. In some places, these stretches are punctuated by whitewater and are perhaps well characterized as rapids, while in others the water flow is smoother.</obo:IAO_0000115>
        <oboInOwl:hasOBONamespace>GAZ</oboInOwl:hasOBONamespace>
        <rdfs:label>Cataracts of the Nile</rdfs:label>
    </rdf:Description>
    <rdf:Description rdf:about="http://purl.obolibrary.org/obo/GAZ_00058886">
        <oboInOwl:id>GAZ:00058886</oboInOwl:id>
        <obo:IAO_0000115>A cataract on the River Nile in the Manasir Desert, Sudan. It will be flooded by the Merowe Dam from 2006.</obo:IAO_0000115>
        <rdfs:label>Fourth Cataract</rdfs:label>
        <oboInOwl:hasOBONamespace>GAZ</oboInOwl:hasOBONamespace>
    </rdf:Description>
    <rdf:Description rdf:about="http://purl.obolibrary.org/obo/GAZ_00058890">
        <rdfs:label>First Cataract</rdfs:label>
        <obo:IAO_0000115>A cataract on the River Nile near Aswan.</obo:IAO_0000115>
        <oboInOwl:hasOBONamespace>GAZ</oboInOwl:hasOBONamespace>
        <oboInOwl:id>GAZ:00058890</oboInOwl:id>
    </rdf:Description>
</rdf:RDF>



<!-- Generated by the OWL API (version 4.5.6) https://github.com/owlcs/owlapi -->

