<?xml version="1.0"?>
<rdf:RDF xmlns="http://purl.obolibrary.org/obo/gaz/subsets/countries/Suriname.owl#"
     xml:base="http://purl.obolibrary.org/obo/gaz/subsets/countries/Suriname.owl"
     xmlns:obo="http://purl.obolibrary.org/obo/"
     xmlns:owl="http://www.w3.org/2002/07/owl#"
     xmlns:rdf="http://www.w3.org/1999/02/22-rdf-syntax-ns#"
     xmlns:xml="http://www.w3.org/XML/1998/namespace"
     xmlns:xsd="http://www.w3.org/2001/XMLSchema#"
     xmlns:rdfs="http://www.w3.org/2000/01/rdf-schema#"
     xmlns:oboInOwl="http://www.geneontology.org/formats/oboInOwl#">
    <owl:Ontology rdf:about="http://purl.obolibrary.org/obo/gaz/subsets/countries/Suriname.owl">
        <owl:imports rdf:resource="http://purl.obolibrary.org/obo/gaz/imports/envo_import.owl"/>
        <owl:imports rdf:resource="http://purl.obolibrary.org/obo/gaz/imports/ro_import.owl"/>
    </owl:Ontology>
    


    <!-- 
    ///////////////////////////////////////////////////////////////////////////////////////
    //
    // Annotation properties
    //
    ///////////////////////////////////////////////////////////////////////////////////////
     -->

    


    <!-- http://purl.obolibrary.org/obo/IAO_0000115 -->

    <owl:AnnotationProperty rdf:about="http://purl.obolibrary.org/obo/IAO_0000115"/>
    


    <!-- http://www.geneontology.org/formats/oboInOwl#hasOBONamespace -->

    <owl:AnnotationProperty rdf:about="http://www.geneontology.org/formats/oboInOwl#hasOBONamespace"/>
    


    <!-- http://www.geneontology.org/formats/oboInOwl#id -->

    <owl:AnnotationProperty rdf:about="http://www.geneontology.org/formats/oboInOwl#id"/>
    


    <!-- 
    ///////////////////////////////////////////////////////////////////////////////////////
    //
    // Object Properties
    //
    ///////////////////////////////////////////////////////////////////////////////////////
     -->

    


    <!-- http://purl.obolibrary.org/obo/RO_0001025 -->

    <owl:ObjectProperty rdf:about="http://purl.obolibrary.org/obo/RO_0001025"/>
    


    <!-- 
    ///////////////////////////////////////////////////////////////////////////////////////
    //
    // Classes
    //
    ///////////////////////////////////////////////////////////////////////////////////////
     -->

    


    <!-- http://purl.obolibrary.org/obo/ENVO_00000009 -->

    <owl:Class rdf:about="http://purl.obolibrary.org/obo/ENVO_00000009"/>
    


    <!-- http://purl.obolibrary.org/obo/ENVO_00000423 -->

    <owl:Class rdf:about="http://purl.obolibrary.org/obo/ENVO_00000423"/>
    


    <!-- http://purl.obolibrary.org/obo/ENVO_00000856 -->

    <owl:Class rdf:about="http://purl.obolibrary.org/obo/ENVO_00000856"/>
    


    <!-- http://purl.obolibrary.org/obo/GAZ_00000082 -->

    <owl:Class rdf:about="http://purl.obolibrary.org/obo/GAZ_00000082">
        <rdfs:subClassOf rdf:resource="http://purl.obolibrary.org/obo/GAZ_00005323"/>
    </owl:Class>
    


    <!-- http://purl.obolibrary.org/obo/GAZ_00000083 -->

    <owl:Class rdf:about="http://purl.obolibrary.org/obo/GAZ_00000083">
        <rdfs:subClassOf rdf:resource="http://purl.obolibrary.org/obo/GAZ_00005322"/>
    </owl:Class>
    


    <!-- http://purl.obolibrary.org/obo/GAZ_00000084 -->

    <owl:Class rdf:about="http://purl.obolibrary.org/obo/GAZ_00000084">
        <rdfs:subClassOf rdf:resource="http://purl.obolibrary.org/obo/GAZ_00005323"/>
    </owl:Class>
    


    <!-- http://purl.obolibrary.org/obo/GAZ_00000085 -->

    <owl:Class rdf:about="http://purl.obolibrary.org/obo/GAZ_00000085">
        <rdfs:subClassOf rdf:resource="http://purl.obolibrary.org/obo/GAZ_00005323"/>
    </owl:Class>
    


    <!-- http://purl.obolibrary.org/obo/GAZ_00000086 -->

    <owl:Class rdf:about="http://purl.obolibrary.org/obo/GAZ_00000086">
        <rdfs:subClassOf rdf:resource="http://purl.obolibrary.org/obo/GAZ_00005323"/>
    </owl:Class>
    


    <!-- http://purl.obolibrary.org/obo/GAZ_00000087 -->

    <owl:Class rdf:about="http://purl.obolibrary.org/obo/GAZ_00000087">
        <rdfs:subClassOf rdf:resource="http://purl.obolibrary.org/obo/GAZ_00005323"/>
    </owl:Class>
    


    <!-- http://purl.obolibrary.org/obo/GAZ_00000088 -->

    <owl:Class rdf:about="http://purl.obolibrary.org/obo/GAZ_00000088">
        <rdfs:subClassOf rdf:resource="http://purl.obolibrary.org/obo/GAZ_00005323"/>
    </owl:Class>
    


    <!-- http://purl.obolibrary.org/obo/GAZ_00000089 -->

    <owl:Class rdf:about="http://purl.obolibrary.org/obo/GAZ_00000089">
        <rdfs:subClassOf rdf:resource="http://purl.obolibrary.org/obo/GAZ_00005323"/>
    </owl:Class>
    


    <!-- http://purl.obolibrary.org/obo/GAZ_00000090 -->

    <owl:Class rdf:about="http://purl.obolibrary.org/obo/GAZ_00000090">
        <rdfs:subClassOf rdf:resource="http://purl.obolibrary.org/obo/GAZ_00005323"/>
    </owl:Class>
    


    <!-- http://purl.obolibrary.org/obo/GAZ_00000091 -->

    <owl:Class rdf:about="http://purl.obolibrary.org/obo/GAZ_00000091">
        <rdfs:subClassOf rdf:resource="http://purl.obolibrary.org/obo/GAZ_00005323"/>
    </owl:Class>
    


    <!-- http://purl.obolibrary.org/obo/GAZ_00000093 -->

    <owl:Class rdf:about="http://purl.obolibrary.org/obo/GAZ_00000093">
        <rdfs:subClassOf rdf:resource="http://purl.obolibrary.org/obo/GAZ_00005322"/>
    </owl:Class>
    


    <!-- http://purl.obolibrary.org/obo/GAZ_00005322 -->

    <owl:Class rdf:about="http://purl.obolibrary.org/obo/GAZ_00005322"/>
    


    <!-- http://purl.obolibrary.org/obo/GAZ_00005323 -->

    <owl:Class rdf:about="http://purl.obolibrary.org/obo/GAZ_00005323"/>
    


    <!-- http://purl.obolibrary.org/obo/GAZ_00005324 -->

    <owl:Class rdf:about="http://purl.obolibrary.org/obo/GAZ_00005324">
        <rdfs:subClassOf rdf:resource="http://purl.obolibrary.org/obo/GAZ_00005323"/>
    </owl:Class>
    


    <!-- http://purl.obolibrary.org/obo/GAZ_00256506 -->

    <owl:Class rdf:about="http://purl.obolibrary.org/obo/GAZ_00256506">
        <rdfs:subClassOf rdf:resource="http://purl.obolibrary.org/obo/GAZ_00005322"/>
    </owl:Class>
    


    <!-- 
    ///////////////////////////////////////////////////////////////////////////////////////
    //
    // Individuals
    //
    ///////////////////////////////////////////////////////////////////////////////////////
     -->

    


    <!-- http://purl.obolibrary.org/obo/GAZ_00000082 -->

    <owl:NamedIndividual rdf:about="http://purl.obolibrary.org/obo/GAZ_00000082"/>
    


    <!-- http://purl.obolibrary.org/obo/GAZ_00000083 -->

    <owl:NamedIndividual rdf:about="http://purl.obolibrary.org/obo/GAZ_00000083">
        <obo:RO_0001025 rdf:resource="http://purl.obolibrary.org/obo/GAZ_00000092"/>
    </owl:NamedIndividual>
    


    <!-- http://purl.obolibrary.org/obo/GAZ_00000084 -->

    <owl:NamedIndividual rdf:about="http://purl.obolibrary.org/obo/GAZ_00000084"/>
    


    <!-- http://purl.obolibrary.org/obo/GAZ_00000085 -->

    <owl:NamedIndividual rdf:about="http://purl.obolibrary.org/obo/GAZ_00000085"/>
    


    <!-- http://purl.obolibrary.org/obo/GAZ_00000086 -->

    <owl:NamedIndividual rdf:about="http://purl.obolibrary.org/obo/GAZ_00000086"/>
    


    <!-- http://purl.obolibrary.org/obo/GAZ_00000087 -->

    <owl:NamedIndividual rdf:about="http://purl.obolibrary.org/obo/GAZ_00000087"/>
    


    <!-- http://purl.obolibrary.org/obo/GAZ_00000088 -->

    <owl:NamedIndividual rdf:about="http://purl.obolibrary.org/obo/GAZ_00000088"/>
    


    <!-- http://purl.obolibrary.org/obo/GAZ_00000089 -->

    <owl:NamedIndividual rdf:about="http://purl.obolibrary.org/obo/GAZ_00000089"/>
    


    <!-- http://purl.obolibrary.org/obo/GAZ_00000090 -->

    <owl:NamedIndividual rdf:about="http://purl.obolibrary.org/obo/GAZ_00000090"/>
    


    <!-- http://purl.obolibrary.org/obo/GAZ_00000091 -->

    <owl:NamedIndividual rdf:about="http://purl.obolibrary.org/obo/GAZ_00000091"/>
    


    <!-- http://purl.obolibrary.org/obo/GAZ_00000092 -->

    <owl:NamedIndividual rdf:about="http://purl.obolibrary.org/obo/GAZ_00000092">
        <obo:RO_0001025 rdf:resource="http://purl.obolibrary.org/obo/GAZ_00000082"/>
        <oboInOwl:hasOBONamespace>GAZ</oboInOwl:hasOBONamespace>
        <oboInOwl:id>GAZ:00000092</oboInOwl:id>
        <rdfs:label>Lelydorp Ressort</rdfs:label>
    </owl:NamedIndividual>
    


    <!-- http://purl.obolibrary.org/obo/GAZ_00000093 -->

    <owl:NamedIndividual rdf:about="http://purl.obolibrary.org/obo/GAZ_00000093">
        <obo:RO_0001025 rdf:resource="http://purl.obolibrary.org/obo/GAZ_00000089"/>
    </owl:NamedIndividual>
    


    <!-- http://purl.obolibrary.org/obo/GAZ_00002525 -->

    <owl:NamedIndividual rdf:about="http://purl.obolibrary.org/obo/GAZ_00002525">
        <rdf:type rdf:resource="http://purl.obolibrary.org/obo/ENVO_00000009"/>
        <obo:IAO_0000115>A country in northern South America. It is situated between French Guiana to the east and Guyana to the west. The southern border is shared with Brazil and the northern border is the Atlantic coast. The southernmost border with French Guiana is disputed along the Marowijne river. Suriname is divided into 10 districts, each of which is divided into Ressorten.</obo:IAO_0000115>
        <oboInOwl:hasOBONamespace>GAZ</oboInOwl:hasOBONamespace>
        <oboInOwl:id>GAZ:00002525</oboInOwl:id>
        <rdfs:label>Suriname</rdfs:label>
    </owl:NamedIndividual>
    


    <!-- http://purl.obolibrary.org/obo/GAZ_00005322 -->

    <owl:NamedIndividual rdf:about="http://purl.obolibrary.org/obo/GAZ_00005322">
        <obo:RO_0001025 rdf:resource="http://purl.obolibrary.org/obo/GAZ_00002525"/>
    </owl:NamedIndividual>
    


    <!-- http://purl.obolibrary.org/obo/GAZ_00005323 -->

    <owl:NamedIndividual rdf:about="http://purl.obolibrary.org/obo/GAZ_00005323">
        <obo:RO_0001025 rdf:resource="http://purl.obolibrary.org/obo/GAZ_00002525"/>
    </owl:NamedIndividual>
    


    <!-- http://purl.obolibrary.org/obo/GAZ_00005324 -->

    <owl:NamedIndividual rdf:about="http://purl.obolibrary.org/obo/GAZ_00005324"/>
    


    <!-- http://purl.obolibrary.org/obo/GAZ_00047130 -->

    <owl:NamedIndividual rdf:about="http://purl.obolibrary.org/obo/GAZ_00047130">
        <obo:IAO_0000115>The largest river in the world by volume, with a total river flow greater than the next top ten largest rivers flowing into the ocean combined.</obo:IAO_0000115>
        <oboInOwl:hasOBONamespace>GAZ</oboInOwl:hasOBONamespace>
        <oboInOwl:id>GAZ:00047130</oboInOwl:id>
        <rdfs:label>River Amazon</rdfs:label>
    </owl:NamedIndividual>
    


    <!-- http://purl.obolibrary.org/obo/GAZ_00047131 -->

    <owl:NamedIndividual rdf:about="http://purl.obolibrary.org/obo/GAZ_00047131">
        <obo:RO_0001025 rdf:resource="http://purl.obolibrary.org/obo/GAZ_00047130"/>
        <obo:IAO_0000115>A complex of broad river channels, islands, mangrove swamps, intertidal mudflats, brackish lagoons and marshes, palm swamps and seasonally flooded grassland and swamp forest. It extends from the SW tip of Ilha Grande de Gurupa 350 km NE to Ilha do Brique, Ilha Janauco, Ilha Caviana, Ilha Mexiana and Western Ilha Marajo.</obo:IAO_0000115>
        <oboInOwl:hasOBONamespace>GAZ</oboInOwl:hasOBONamespace>
        <oboInOwl:id>GAZ:00047131</oboInOwl:id>
        <rdfs:label>River Amazon Delta</rdfs:label>
    </owl:NamedIndividual>
    


    <!-- http://purl.obolibrary.org/obo/GAZ_00047132 -->

    <owl:NamedIndividual rdf:about="http://purl.obolibrary.org/obo/GAZ_00047132">
        <obo:RO_0001025 rdf:resource="http://purl.obolibrary.org/obo/GAZ_00047131"/>
        <obo:IAO_0000115>An island located at the mouth of the Amazon River in Brazil. It is part of the State of Para. It is the largest island to be completely surrounded by freshwater in the world. Although its northeast coastline faces the Atlantic Ocean, the outflow from the Amazon is so great that the sea at the mouth is quite unbriny for some distance from shore. The city of Belem lies to the south, across the southern fork (also called the Para River) of the river&apos;s mouth. The island sits almost directly on the equator.</obo:IAO_0000115>
        <oboInOwl:hasOBONamespace>GAZ</oboInOwl:hasOBONamespace>
        <oboInOwl:id>GAZ:00047132</oboInOwl:id>
        <rdfs:label>Ilha de Marajo</rdfs:label>
    </owl:NamedIndividual>
    


    <!-- http://purl.obolibrary.org/obo/GAZ_00049223 -->

    <owl:NamedIndividual rdf:about="http://purl.obolibrary.org/obo/GAZ_00049223">
        <obo:IAO_0000115>The largest left tributary of the Amazon and the largest blackwater river in the world. It has its sources along the watershed between the Orinoco and the Amazon basins, and also connects with the Orinoco by way of the Casiquiare canal. In Colombia, where their sources are, it is called the Guainia River. Its main affluent is Vaupes, which disputes with the headwaters of the Guaviare branch of the Orinoco, the drainage of the eastern slope of the Andes of Colombia. The Rio Negro flows into the Rio Solimoes to form the Amazon River near Manaus, Brazil.</obo:IAO_0000115>
        <oboInOwl:hasOBONamespace>GAZ</oboInOwl:hasOBONamespace>
        <oboInOwl:id>GAZ:00049223</oboInOwl:id>
        <rdfs:label>Rio Negro</rdfs:label>
    </owl:NamedIndividual>
    


    <!-- http://purl.obolibrary.org/obo/GAZ_00049224 -->

    <owl:NamedIndividual rdf:about="http://purl.obolibrary.org/obo/GAZ_00049224">
        <obo:RO_0001025 rdf:resource="http://purl.obolibrary.org/obo/GAZ_00049223"/>
        <obo:IAO_0000115>An island split between Brazil and Colombia.</obo:IAO_0000115>
        <oboInOwl:hasOBONamespace>GAZ</oboInOwl:hasOBONamespace>
        <oboInOwl:id>GAZ:00049224</oboInOwl:id>
        <rdfs:label>San Jose Island</rdfs:label>
    </owl:NamedIndividual>
    


    <!-- http://purl.obolibrary.org/obo/GAZ_00056739 -->

    <owl:NamedIndividual rdf:about="http://purl.obolibrary.org/obo/GAZ_00056739">
        <obo:RO_0001025 rdf:resource="http://purl.obolibrary.org/obo/GAZ_00000091"/>
        <obo:IAO_0000115>A mountain range in Suriname.</obo:IAO_0000115>
        <oboInOwl:hasOBONamespace>GAZ</oboInOwl:hasOBONamespace>
        <oboInOwl:id>GAZ:00056739</oboInOwl:id>
        <rdfs:label>Bakhuys Mountains</rdfs:label>
    </owl:NamedIndividual>
    


    <!-- http://purl.obolibrary.org/obo/GAZ_00056740 -->

    <owl:NamedIndividual rdf:about="http://purl.obolibrary.org/obo/GAZ_00056740">
        <obo:RO_0001025 rdf:resource="http://purl.obolibrary.org/obo/GAZ_00000091"/>
        <obo:IAO_0000115>A mountain range in Suriname.</obo:IAO_0000115>
        <oboInOwl:hasOBONamespace>GAZ</oboInOwl:hasOBONamespace>
        <oboInOwl:id>GAZ:00056740</oboInOwl:id>
        <rdfs:label>Van Asch Van Wijck Mountains</rdfs:label>
    </owl:NamedIndividual>
    


    <!-- http://purl.obolibrary.org/obo/GAZ_00056742 -->

    <owl:NamedIndividual rdf:about="http://purl.obolibrary.org/obo/GAZ_00056742">
        <obo:RO_0001025 rdf:resource="http://purl.obolibrary.org/obo/GAZ_00002525"/>
        <obo:IAO_0000115>A protected region that contains 16,000 km2 of both montane and lowland primary tropical forest including sections of the Guyana Highlands. A World Heritage Site.</obo:IAO_0000115>
        <oboInOwl:hasOBONamespace>GAZ</oboInOwl:hasOBONamespace>
        <oboInOwl:id>GAZ:00056742</oboInOwl:id>
        <rdfs:label>Central Suriname Nature Reserve</rdfs:label>
    </owl:NamedIndividual>
    


    <!-- http://purl.obolibrary.org/obo/GAZ_00067322 -->

    <owl:NamedIndividual rdf:about="http://purl.obolibrary.org/obo/GAZ_00067322">
        <obo:RO_0001025 rdf:resource="http://purl.obolibrary.org/obo/GAZ_00000084"/>
        <oboInOwl:hasOBONamespace>GAZ</oboInOwl:hasOBONamespace>
        <oboInOwl:id>GAZ:00067322</oboInOwl:id>
        <rdfs:label>Marshallkreek Ressort</rdfs:label>
    </owl:NamedIndividual>
    


    <!-- http://purl.obolibrary.org/obo/GAZ_00067323 -->

    <owl:NamedIndividual rdf:about="http://purl.obolibrary.org/obo/GAZ_00067323">
        <obo:RO_0001025 rdf:resource="http://purl.obolibrary.org/obo/GAZ_00000084"/>
        <oboInOwl:hasOBONamespace>GAZ</oboInOwl:hasOBONamespace>
        <oboInOwl:id>GAZ:00067323</oboInOwl:id>
        <rdfs:label>Centrum Ressort</rdfs:label>
    </owl:NamedIndividual>
    


    <!-- http://purl.obolibrary.org/obo/GAZ_00067324 -->

    <owl:NamedIndividual rdf:about="http://purl.obolibrary.org/obo/GAZ_00067324">
        <obo:RO_0001025 rdf:resource="http://purl.obolibrary.org/obo/GAZ_00000084"/>
        <oboInOwl:hasOBONamespace>GAZ</oboInOwl:hasOBONamespace>
        <oboInOwl:id>GAZ:00067324</oboInOwl:id>
        <rdfs:label>Sarakreek Ressort</rdfs:label>
    </owl:NamedIndividual>
    


    <!-- http://purl.obolibrary.org/obo/GAZ_00067325 -->

    <owl:NamedIndividual rdf:about="http://purl.obolibrary.org/obo/GAZ_00067325">
        <obo:RO_0001025 rdf:resource="http://purl.obolibrary.org/obo/GAZ_00000084"/>
        <oboInOwl:hasOBONamespace>GAZ</oboInOwl:hasOBONamespace>
        <oboInOwl:id>GAZ:00067325</oboInOwl:id>
        <rdfs:label>Brownsweg Ressort</rdfs:label>
    </owl:NamedIndividual>
    


    <!-- http://purl.obolibrary.org/obo/GAZ_00067326 -->

    <owl:NamedIndividual rdf:about="http://purl.obolibrary.org/obo/GAZ_00067326">
        <obo:RO_0001025 rdf:resource="http://purl.obolibrary.org/obo/GAZ_00000084"/>
        <oboInOwl:hasOBONamespace>GAZ</oboInOwl:hasOBONamespace>
        <oboInOwl:id>GAZ:00067326</oboInOwl:id>
        <rdfs:label>Klaaskreek Ressort</rdfs:label>
    </owl:NamedIndividual>
    


    <!-- http://purl.obolibrary.org/obo/GAZ_00067327 -->

    <owl:NamedIndividual rdf:about="http://purl.obolibrary.org/obo/GAZ_00067327">
        <obo:RO_0001025 rdf:resource="http://purl.obolibrary.org/obo/GAZ_00000084"/>
        <oboInOwl:hasOBONamespace>GAZ</oboInOwl:hasOBONamespace>
        <oboInOwl:id>GAZ:00067327</oboInOwl:id>
        <rdfs:label>Kwakoegron Ressort</rdfs:label>
    </owl:NamedIndividual>
    


    <!-- http://purl.obolibrary.org/obo/GAZ_00067328 -->

    <owl:NamedIndividual rdf:about="http://purl.obolibrary.org/obo/GAZ_00067328">
        <obo:RO_0001025 rdf:resource="http://purl.obolibrary.org/obo/GAZ_00000085"/>
        <oboInOwl:hasOBONamespace>GAZ</oboInOwl:hasOBONamespace>
        <oboInOwl:id>GAZ:00067328</oboInOwl:id>
        <rdfs:label>Nieuw Amsterdam Ressort</rdfs:label>
    </owl:NamedIndividual>
    


    <!-- http://purl.obolibrary.org/obo/GAZ_00067329 -->

    <owl:NamedIndividual rdf:about="http://purl.obolibrary.org/obo/GAZ_00067329">
        <obo:RO_0001025 rdf:resource="http://purl.obolibrary.org/obo/GAZ_00000085"/>
        <oboInOwl:hasOBONamespace>GAZ</oboInOwl:hasOBONamespace>
        <oboInOwl:id>GAZ:00067329</oboInOwl:id>
        <rdfs:label>Bakkie Ressort</rdfs:label>
    </owl:NamedIndividual>
    


    <!-- http://purl.obolibrary.org/obo/GAZ_00067330 -->

    <owl:NamedIndividual rdf:about="http://purl.obolibrary.org/obo/GAZ_00067330">
        <obo:RO_0001025 rdf:resource="http://purl.obolibrary.org/obo/GAZ_00000085"/>
        <oboInOwl:hasOBONamespace>GAZ</oboInOwl:hasOBONamespace>
        <oboInOwl:id>GAZ:00067330</oboInOwl:id>
        <rdfs:label>Tamanredjo Ressort</rdfs:label>
    </owl:NamedIndividual>
    


    <!-- http://purl.obolibrary.org/obo/GAZ_00067331 -->

    <owl:NamedIndividual rdf:about="http://purl.obolibrary.org/obo/GAZ_00067331">
        <obo:RO_0001025 rdf:resource="http://purl.obolibrary.org/obo/GAZ_00000085"/>
        <oboInOwl:hasOBONamespace>GAZ</oboInOwl:hasOBONamespace>
        <oboInOwl:id>GAZ:00067331</oboInOwl:id>
        <rdfs:label>Meerzorg Ressort</rdfs:label>
    </owl:NamedIndividual>
    


    <!-- http://purl.obolibrary.org/obo/GAZ_00067332 -->

    <owl:NamedIndividual rdf:about="http://purl.obolibrary.org/obo/GAZ_00067332">
        <obo:RO_0001025 rdf:resource="http://purl.obolibrary.org/obo/GAZ_00000085"/>
        <oboInOwl:hasOBONamespace>GAZ</oboInOwl:hasOBONamespace>
        <oboInOwl:id>GAZ:00067332</oboInOwl:id>
        <rdfs:label>Alkmaar Ressort</rdfs:label>
    </owl:NamedIndividual>
    


    <!-- http://purl.obolibrary.org/obo/GAZ_00067333 -->

    <owl:NamedIndividual rdf:about="http://purl.obolibrary.org/obo/GAZ_00067333">
        <obo:RO_0001025 rdf:resource="http://purl.obolibrary.org/obo/GAZ_00000085"/>
        <oboInOwl:hasOBONamespace>GAZ</oboInOwl:hasOBONamespace>
        <oboInOwl:id>GAZ:00067333</oboInOwl:id>
        <rdfs:label>Margaretha Ressort</rdfs:label>
    </owl:NamedIndividual>
    


    <!-- http://purl.obolibrary.org/obo/GAZ_00067334 -->

    <owl:NamedIndividual rdf:about="http://purl.obolibrary.org/obo/GAZ_00067334">
        <obo:RO_0001025 rdf:resource="http://purl.obolibrary.org/obo/GAZ_00000086"/>
        <oboInOwl:hasOBONamespace>GAZ</oboInOwl:hasOBONamespace>
        <oboInOwl:id>GAZ:00067334</oboInOwl:id>
        <rdfs:label>Totness Ressort</rdfs:label>
    </owl:NamedIndividual>
    


    <!-- http://purl.obolibrary.org/obo/GAZ_00067335 -->

    <owl:NamedIndividual rdf:about="http://purl.obolibrary.org/obo/GAZ_00067335">
        <obo:RO_0001025 rdf:resource="http://purl.obolibrary.org/obo/GAZ_00000086"/>
        <oboInOwl:hasOBONamespace>GAZ</oboInOwl:hasOBONamespace>
        <oboInOwl:id>GAZ:00067335</oboInOwl:id>
        <rdfs:label>Johanna Maria Ressort</rdfs:label>
    </owl:NamedIndividual>
    


    <!-- http://purl.obolibrary.org/obo/GAZ_00067336 -->

    <owl:NamedIndividual rdf:about="http://purl.obolibrary.org/obo/GAZ_00067336">
        <obo:RO_0001025 rdf:resource="http://purl.obolibrary.org/obo/GAZ_00000086"/>
        <oboInOwl:hasOBONamespace>GAZ</oboInOwl:hasOBONamespace>
        <oboInOwl:id>GAZ:00067336</oboInOwl:id>
        <rdfs:label>Welgelegen Ressort</rdfs:label>
    </owl:NamedIndividual>
    


    <!-- http://purl.obolibrary.org/obo/GAZ_00067337 -->

    <owl:NamedIndividual rdf:about="http://purl.obolibrary.org/obo/GAZ_00067337">
        <obo:RO_0001025 rdf:resource="http://purl.obolibrary.org/obo/GAZ_00000084"/>
        <obo:IAO_0000115>A large reservoir in the South American country of Suriname. The reservoir was created by constructing a dam across the Suriname River between 1961 and 1964.</obo:IAO_0000115>
        <oboInOwl:hasOBONamespace>GAZ</oboInOwl:hasOBONamespace>
        <oboInOwl:id>GAZ:00067337</oboInOwl:id>
        <rdfs:label>Brokopondo Reservoir</rdfs:label>
    </owl:NamedIndividual>
    


    <!-- http://purl.obolibrary.org/obo/GAZ_00067339 -->

    <owl:NamedIndividual rdf:about="http://purl.obolibrary.org/obo/GAZ_00067339">
        <obo:RO_0001025 rdf:resource="http://purl.obolibrary.org/obo/GAZ_00000091"/>
        <obo:IAO_0000115>A mountain range in central Suriname that extends about 113 km from west to east. Its highest peak is Julianatop with 1280 m. The Wilhelmina Mountains are part of the Tumucumaque Uplands of the Guiana Shield.</obo:IAO_0000115>
        <oboInOwl:hasOBONamespace>GAZ</oboInOwl:hasOBONamespace>
        <oboInOwl:id>GAZ:00067339</oboInOwl:id>
        <rdfs:label>Wilhelmina Mountains</rdfs:label>
    </owl:NamedIndividual>
    


    <!-- http://purl.obolibrary.org/obo/GAZ_00067340 -->

    <owl:NamedIndividual rdf:about="http://purl.obolibrary.org/obo/GAZ_00067340">
        <obo:RO_0001025 rdf:resource="http://purl.obolibrary.org/obo/GAZ_00000091"/>
        <obo:IAO_0000115>A mountain range in Sipaliwini District, Suriname, It is a southern part of Wilhelmina Mountains and is maximum 986 m high.</obo:IAO_0000115>
        <oboInOwl:hasOBONamespace>GAZ</oboInOwl:hasOBONamespace>
        <oboInOwl:id>GAZ:00067340</oboInOwl:id>
        <rdfs:label>Eilerts de Haan Mountains</rdfs:label>
    </owl:NamedIndividual>
    


    <!-- http://purl.obolibrary.org/obo/GAZ_00067341 -->

    <owl:NamedIndividual rdf:about="http://purl.obolibrary.org/obo/GAZ_00067341">
        <obo:RO_0001025 rdf:resource="http://purl.obolibrary.org/obo/GAZ_00000087"/>
        <oboInOwl:hasOBONamespace>GAZ</oboInOwl:hasOBONamespace>
        <oboInOwl:id>GAZ:00067341</oboInOwl:id>
        <rdfs:label>Moengo Ressort</rdfs:label>
    </owl:NamedIndividual>
    


    <!-- http://purl.obolibrary.org/obo/GAZ_00067342 -->

    <owl:NamedIndividual rdf:about="http://purl.obolibrary.org/obo/GAZ_00067342">
        <obo:RO_0001025 rdf:resource="http://purl.obolibrary.org/obo/GAZ_00000087"/>
        <oboInOwl:hasOBONamespace>GAZ</oboInOwl:hasOBONamespace>
        <oboInOwl:id>GAZ:00067342</oboInOwl:id>
        <rdfs:label>Albina Ressort</rdfs:label>
    </owl:NamedIndividual>
    


    <!-- http://purl.obolibrary.org/obo/GAZ_00067343 -->

    <owl:NamedIndividual rdf:about="http://purl.obolibrary.org/obo/GAZ_00067343">
        <obo:RO_0001025 rdf:resource="http://purl.obolibrary.org/obo/GAZ_00000087"/>
        <oboInOwl:hasOBONamespace>GAZ</oboInOwl:hasOBONamespace>
        <oboInOwl:id>GAZ:00067343</oboInOwl:id>
        <rdfs:label>Wanhatti Ressort</rdfs:label>
    </owl:NamedIndividual>
    


    <!-- http://purl.obolibrary.org/obo/GAZ_00067344 -->

    <owl:NamedIndividual rdf:about="http://purl.obolibrary.org/obo/GAZ_00067344">
        <obo:RO_0001025 rdf:resource="http://purl.obolibrary.org/obo/GAZ_00000087"/>
        <oboInOwl:hasOBONamespace>GAZ</oboInOwl:hasOBONamespace>
        <oboInOwl:id>GAZ:00067344</oboInOwl:id>
        <rdfs:label>Galibi Ressort</rdfs:label>
    </owl:NamedIndividual>
    


    <!-- http://purl.obolibrary.org/obo/GAZ_00067345 -->

    <owl:NamedIndividual rdf:about="http://purl.obolibrary.org/obo/GAZ_00067345">
        <obo:RO_0001025 rdf:resource="http://purl.obolibrary.org/obo/GAZ_00000087"/>
        <oboInOwl:hasOBONamespace>GAZ</oboInOwl:hasOBONamespace>
        <oboInOwl:id>GAZ:00067345</oboInOwl:id>
        <rdfs:label>Moengotapoe Ressort</rdfs:label>
    </owl:NamedIndividual>
    


    <!-- http://purl.obolibrary.org/obo/GAZ_00067346 -->

    <owl:NamedIndividual rdf:about="http://purl.obolibrary.org/obo/GAZ_00067346">
        <obo:RO_0001025 rdf:resource="http://purl.obolibrary.org/obo/GAZ_00000087"/>
        <oboInOwl:hasOBONamespace>GAZ</oboInOwl:hasOBONamespace>
        <oboInOwl:id>GAZ:00067346</oboInOwl:id>
        <rdfs:label>Patamacca Ressort</rdfs:label>
    </owl:NamedIndividual>
    


    <!-- http://purl.obolibrary.org/obo/GAZ_00067347 -->

    <owl:NamedIndividual rdf:about="http://purl.obolibrary.org/obo/GAZ_00067347">
        <obo:RO_0001025 rdf:resource="http://purl.obolibrary.org/obo/GAZ_00000088"/>
        <obo:IAO_0000115>A community ressort and an agricultural place in the Republic of Suriname and located in the coastal area of West Suriname in the Nickerie District, at the harbour of the Nickerie river across the right estuary of the Maratakka river.</obo:IAO_0000115>
        <oboInOwl:hasOBONamespace>GAZ</oboInOwl:hasOBONamespace>
        <oboInOwl:id>GAZ:00067347</oboInOwl:id>
        <rdfs:label>Wageningen Ressort</rdfs:label>
    </owl:NamedIndividual>
    


    <!-- http://purl.obolibrary.org/obo/GAZ_00067348 -->

    <owl:NamedIndividual rdf:about="http://purl.obolibrary.org/obo/GAZ_00067348">
        <obo:RO_0001025 rdf:resource="http://purl.obolibrary.org/obo/GAZ_00000088"/>
        <oboInOwl:hasOBONamespace>GAZ</oboInOwl:hasOBONamespace>
        <oboInOwl:id>GAZ:00067348</oboInOwl:id>
        <rdfs:label>Nieuw Nickerie Ressort</rdfs:label>
    </owl:NamedIndividual>
    


    <!-- http://purl.obolibrary.org/obo/GAZ_00067349 -->

    <owl:NamedIndividual rdf:about="http://purl.obolibrary.org/obo/GAZ_00067349">
        <obo:RO_0001025 rdf:resource="http://purl.obolibrary.org/obo/GAZ_00000088"/>
        <oboInOwl:hasOBONamespace>GAZ</oboInOwl:hasOBONamespace>
        <oboInOwl:id>GAZ:00067349</oboInOwl:id>
        <rdfs:label>Westelijke Polders Ressort</rdfs:label>
    </owl:NamedIndividual>
    


    <!-- http://purl.obolibrary.org/obo/GAZ_00067350 -->

    <owl:NamedIndividual rdf:about="http://purl.obolibrary.org/obo/GAZ_00067350">
        <obo:RO_0001025 rdf:resource="http://purl.obolibrary.org/obo/GAZ_00000088"/>
        <oboInOwl:hasOBONamespace>GAZ</oboInOwl:hasOBONamespace>
        <oboInOwl:id>GAZ:00067350</oboInOwl:id>
        <rdfs:label>Groot Henar Ressort</rdfs:label>
    </owl:NamedIndividual>
    


    <!-- http://purl.obolibrary.org/obo/GAZ_00067351 -->

    <owl:NamedIndividual rdf:about="http://purl.obolibrary.org/obo/GAZ_00067351">
        <obo:RO_0001025 rdf:resource="http://purl.obolibrary.org/obo/GAZ_00000088"/>
        <oboInOwl:hasOBONamespace>GAZ</oboInOwl:hasOBONamespace>
        <oboInOwl:id>GAZ:00067351</oboInOwl:id>
        <rdfs:label>Oostelijke Polders Ressort</rdfs:label>
    </owl:NamedIndividual>
    


    <!-- http://purl.obolibrary.org/obo/GAZ_00067352 -->

    <owl:NamedIndividual rdf:about="http://purl.obolibrary.org/obo/GAZ_00067352">
        <obo:RO_0001025 rdf:resource="http://purl.obolibrary.org/obo/GAZ_00000089"/>
        <oboInOwl:hasOBONamespace>GAZ</oboInOwl:hasOBONamespace>
        <oboInOwl:id>GAZ:00067352</oboInOwl:id>
        <rdfs:label>Noord-Para Ressort</rdfs:label>
    </owl:NamedIndividual>
    


    <!-- http://purl.obolibrary.org/obo/GAZ_00067353 -->

    <owl:NamedIndividual rdf:about="http://purl.obolibrary.org/obo/GAZ_00067353">
        <obo:RO_0001025 rdf:resource="http://purl.obolibrary.org/obo/GAZ_00000089"/>
        <oboInOwl:hasOBONamespace>GAZ</oboInOwl:hasOBONamespace>
        <oboInOwl:id>GAZ:00067353</oboInOwl:id>
        <rdfs:label>Zuid-Para Ressort</rdfs:label>
    </owl:NamedIndividual>
    


    <!-- http://purl.obolibrary.org/obo/GAZ_00067354 -->

    <owl:NamedIndividual rdf:about="http://purl.obolibrary.org/obo/GAZ_00067354">
        <obo:RO_0001025 rdf:resource="http://purl.obolibrary.org/obo/GAZ_00000089"/>
        <oboInOwl:hasOBONamespace>GAZ</oboInOwl:hasOBONamespace>
        <oboInOwl:id>GAZ:00067354</oboInOwl:id>
        <rdfs:label>Bigi Poika Ressort</rdfs:label>
    </owl:NamedIndividual>
    


    <!-- http://purl.obolibrary.org/obo/GAZ_00067355 -->

    <owl:NamedIndividual rdf:about="http://purl.obolibrary.org/obo/GAZ_00067355">
        <obo:RO_0001025 rdf:resource="http://purl.obolibrary.org/obo/GAZ_00000089"/>
        <oboInOwl:hasOBONamespace>GAZ</oboInOwl:hasOBONamespace>
        <oboInOwl:id>GAZ:00067355</oboInOwl:id>
        <rdfs:label>Oost-Para Ressort</rdfs:label>
    </owl:NamedIndividual>
    


    <!-- http://purl.obolibrary.org/obo/GAZ_00067356 -->

    <owl:NamedIndividual rdf:about="http://purl.obolibrary.org/obo/GAZ_00067356">
        <obo:RO_0001025 rdf:resource="http://purl.obolibrary.org/obo/GAZ_00000089"/>
        <oboInOwl:hasOBONamespace>GAZ</oboInOwl:hasOBONamespace>
        <oboInOwl:id>GAZ:00067356</oboInOwl:id>
        <rdfs:label>Carolina Ressort</rdfs:label>
    </owl:NamedIndividual>
    


    <!-- http://purl.obolibrary.org/obo/GAZ_00067357 -->

    <owl:NamedIndividual rdf:about="http://purl.obolibrary.org/obo/GAZ_00067357">
        <obo:RO_0001025 rdf:resource="http://purl.obolibrary.org/obo/GAZ_00005324"/>
        <oboInOwl:hasOBONamespace>GAZ</oboInOwl:hasOBONamespace>
        <oboInOwl:id>GAZ:00067357</oboInOwl:id>
        <rdfs:label>Flora Ressort</rdfs:label>
    </owl:NamedIndividual>
    


    <!-- http://purl.obolibrary.org/obo/GAZ_00067358 -->

    <owl:NamedIndividual rdf:about="http://purl.obolibrary.org/obo/GAZ_00067358">
        <obo:RO_0001025 rdf:resource="http://purl.obolibrary.org/obo/GAZ_00005324"/>
        <oboInOwl:hasOBONamespace>GAZ</oboInOwl:hasOBONamespace>
        <oboInOwl:id>GAZ:00067358</oboInOwl:id>
        <rdfs:label>Blauwgrond Ressort</rdfs:label>
    </owl:NamedIndividual>
    


    <!-- http://purl.obolibrary.org/obo/GAZ_00067359 -->

    <owl:NamedIndividual rdf:about="http://purl.obolibrary.org/obo/GAZ_00067359">
        <obo:RO_0001025 rdf:resource="http://purl.obolibrary.org/obo/GAZ_00005324"/>
        <oboInOwl:hasOBONamespace>GAZ</oboInOwl:hasOBONamespace>
        <oboInOwl:id>GAZ:00067359</oboInOwl:id>
        <rdfs:label>Wegnaarzee Ressort</rdfs:label>
    </owl:NamedIndividual>
    


    <!-- http://purl.obolibrary.org/obo/GAZ_00067360 -->

    <owl:NamedIndividual rdf:about="http://purl.obolibrary.org/obo/GAZ_00067360">
        <obo:RO_0001025 rdf:resource="http://purl.obolibrary.org/obo/GAZ_00005324"/>
        <oboInOwl:hasOBONamespace>GAZ</oboInOwl:hasOBONamespace>
        <oboInOwl:id>GAZ:00067360</oboInOwl:id>
        <rdfs:label>Pontbuiten Ressort</rdfs:label>
    </owl:NamedIndividual>
    


    <!-- http://purl.obolibrary.org/obo/GAZ_00067361 -->

    <owl:NamedIndividual rdf:about="http://purl.obolibrary.org/obo/GAZ_00067361">
        <obo:RO_0001025 rdf:resource="http://purl.obolibrary.org/obo/GAZ_00005324"/>
        <oboInOwl:hasOBONamespace>GAZ</oboInOwl:hasOBONamespace>
        <oboInOwl:id>GAZ:00067361</oboInOwl:id>
        <rdfs:label>Latour Ressort</rdfs:label>
    </owl:NamedIndividual>
    


    <!-- http://purl.obolibrary.org/obo/GAZ_00067362 -->

    <owl:NamedIndividual rdf:about="http://purl.obolibrary.org/obo/GAZ_00067362">
        <obo:RO_0001025 rdf:resource="http://purl.obolibrary.org/obo/GAZ_00005324"/>
        <oboInOwl:hasOBONamespace>GAZ</oboInOwl:hasOBONamespace>
        <oboInOwl:id>GAZ:00067362</oboInOwl:id>
        <rdfs:label>Rainville Ressort</rdfs:label>
    </owl:NamedIndividual>
    


    <!-- http://purl.obolibrary.org/obo/GAZ_00067363 -->

    <owl:NamedIndividual rdf:about="http://purl.obolibrary.org/obo/GAZ_00067363">
        <obo:RO_0001025 rdf:resource="http://purl.obolibrary.org/obo/GAZ_00005324"/>
        <oboInOwl:hasOBONamespace>GAZ</oboInOwl:hasOBONamespace>
        <oboInOwl:id>GAZ:00067363</oboInOwl:id>
        <rdfs:label>Tammenga Ressort</rdfs:label>
    </owl:NamedIndividual>
    


    <!-- http://purl.obolibrary.org/obo/GAZ_00067364 -->

    <owl:NamedIndividual rdf:about="http://purl.obolibrary.org/obo/GAZ_00067364">
        <obo:RO_0001025 rdf:resource="http://purl.obolibrary.org/obo/GAZ_00005324"/>
        <oboInOwl:hasOBONamespace>GAZ</oboInOwl:hasOBONamespace>
        <oboInOwl:id>GAZ:00067364</oboInOwl:id>
        <rdfs:label>Welgelegen Ressort</rdfs:label>
    </owl:NamedIndividual>
    


    <!-- http://purl.obolibrary.org/obo/GAZ_00067365 -->

    <owl:NamedIndividual rdf:about="http://purl.obolibrary.org/obo/GAZ_00067365">
        <obo:RO_0001025 rdf:resource="http://purl.obolibrary.org/obo/GAZ_00005324"/>
        <oboInOwl:hasOBONamespace>GAZ</oboInOwl:hasOBONamespace>
        <oboInOwl:id>GAZ:00067365</oboInOwl:id>
        <rdfs:label>Livorno Ressort</rdfs:label>
    </owl:NamedIndividual>
    


    <!-- http://purl.obolibrary.org/obo/GAZ_00067366 -->

    <owl:NamedIndividual rdf:about="http://purl.obolibrary.org/obo/GAZ_00067366">
        <obo:RO_0001025 rdf:resource="http://purl.obolibrary.org/obo/GAZ_00005324"/>
        <oboInOwl:hasOBONamespace>GAZ</oboInOwl:hasOBONamespace>
        <oboInOwl:id>GAZ:00067366</oboInOwl:id>
        <rdfs:label>Munder Ressort</rdfs:label>
    </owl:NamedIndividual>
    


    <!-- http://purl.obolibrary.org/obo/GAZ_00067367 -->

    <owl:NamedIndividual rdf:about="http://purl.obolibrary.org/obo/GAZ_00067367">
        <obo:RO_0001025 rdf:resource="http://purl.obolibrary.org/obo/GAZ_00005324"/>
        <oboInOwl:hasOBONamespace>GAZ</oboInOwl:hasOBONamespace>
        <oboInOwl:id>GAZ:00067367</oboInOwl:id>
        <rdfs:label>Zorg en Hoop Ressort</rdfs:label>
    </owl:NamedIndividual>
    


    <!-- http://purl.obolibrary.org/obo/GAZ_00067368 -->

    <owl:NamedIndividual rdf:about="http://purl.obolibrary.org/obo/GAZ_00067368">
        <obo:RO_0001025 rdf:resource="http://purl.obolibrary.org/obo/GAZ_00005324"/>
        <oboInOwl:hasOBONamespace>GAZ</oboInOwl:hasOBONamespace>
        <oboInOwl:id>GAZ:00067368</oboInOwl:id>
        <rdfs:label>Beekhuizen Ressort</rdfs:label>
    </owl:NamedIndividual>
    


    <!-- http://purl.obolibrary.org/obo/GAZ_00067369 -->

    <owl:NamedIndividual rdf:about="http://purl.obolibrary.org/obo/GAZ_00067369">
        <obo:RO_0001025 rdf:resource="http://purl.obolibrary.org/obo/GAZ_00005324"/>
        <oboInOwl:hasOBONamespace>GAZ</oboInOwl:hasOBONamespace>
        <oboInOwl:id>GAZ:00067369</oboInOwl:id>
        <rdfs:label>Maretraite Ressort</rdfs:label>
    </owl:NamedIndividual>
    


    <!-- http://purl.obolibrary.org/obo/GAZ_00067370 -->

    <owl:NamedIndividual rdf:about="http://purl.obolibrary.org/obo/GAZ_00067370">
        <obo:RO_0001025 rdf:resource="http://purl.obolibrary.org/obo/GAZ_00005324"/>
        <oboInOwl:hasOBONamespace>GAZ</oboInOwl:hasOBONamespace>
        <oboInOwl:id>GAZ:00067370</oboInOwl:id>
        <rdfs:label>Centrum Ressort</rdfs:label>
    </owl:NamedIndividual>
    


    <!-- http://purl.obolibrary.org/obo/GAZ_00067371 -->

    <owl:NamedIndividual rdf:about="http://purl.obolibrary.org/obo/GAZ_00067371">
        <obo:RO_0001025 rdf:resource="http://purl.obolibrary.org/obo/GAZ_00000090"/>
        <oboInOwl:hasOBONamespace>GAZ</oboInOwl:hasOBONamespace>
        <oboInOwl:id>GAZ:00067371</oboInOwl:id>
        <rdfs:label>Kampong Baroe Ressort</rdfs:label>
    </owl:NamedIndividual>
    


    <!-- http://purl.obolibrary.org/obo/GAZ_00067372 -->

    <owl:NamedIndividual rdf:about="http://purl.obolibrary.org/obo/GAZ_00067372">
        <obo:RO_0001025 rdf:resource="http://purl.obolibrary.org/obo/GAZ_00000090"/>
        <oboInOwl:hasOBONamespace>GAZ</oboInOwl:hasOBONamespace>
        <oboInOwl:id>GAZ:00067372</oboInOwl:id>
        <rdfs:label>Jarikaba Ressort</rdfs:label>
    </owl:NamedIndividual>
    


    <!-- http://purl.obolibrary.org/obo/GAZ_00067373 -->

    <owl:NamedIndividual rdf:about="http://purl.obolibrary.org/obo/GAZ_00067373">
        <obo:RO_0001025 rdf:resource="http://purl.obolibrary.org/obo/GAZ_00000090"/>
        <oboInOwl:hasOBONamespace>GAZ</oboInOwl:hasOBONamespace>
        <oboInOwl:id>GAZ:00067373</oboInOwl:id>
        <rdfs:label>Wayamboweg Ressort</rdfs:label>
    </owl:NamedIndividual>
    


    <!-- http://purl.obolibrary.org/obo/GAZ_00067374 -->

    <owl:NamedIndividual rdf:about="http://purl.obolibrary.org/obo/GAZ_00067374">
        <obo:RO_0001025 rdf:resource="http://purl.obolibrary.org/obo/GAZ_00000090"/>
        <oboInOwl:hasOBONamespace>GAZ</oboInOwl:hasOBONamespace>
        <oboInOwl:id>GAZ:00067374</oboInOwl:id>
        <rdfs:label>Tijgerkreek Ressort</rdfs:label>
    </owl:NamedIndividual>
    


    <!-- http://purl.obolibrary.org/obo/GAZ_00067375 -->

    <owl:NamedIndividual rdf:about="http://purl.obolibrary.org/obo/GAZ_00067375">
        <obo:RO_0001025 rdf:resource="http://purl.obolibrary.org/obo/GAZ_00000090"/>
        <oboInOwl:hasOBONamespace>GAZ</oboInOwl:hasOBONamespace>
        <oboInOwl:id>GAZ:00067375</oboInOwl:id>
        <rdfs:label>Calcutta Ressort</rdfs:label>
    </owl:NamedIndividual>
    


    <!-- http://purl.obolibrary.org/obo/GAZ_00067376 -->

    <owl:NamedIndividual rdf:about="http://purl.obolibrary.org/obo/GAZ_00067376">
        <obo:RO_0001025 rdf:resource="http://purl.obolibrary.org/obo/GAZ_00000090"/>
        <oboInOwl:hasOBONamespace>GAZ</oboInOwl:hasOBONamespace>
        <oboInOwl:id>GAZ:00067376</oboInOwl:id>
        <rdfs:label>Groningen Ressort</rdfs:label>
    </owl:NamedIndividual>
    


    <!-- http://purl.obolibrary.org/obo/GAZ_00067377 -->

    <owl:NamedIndividual rdf:about="http://purl.obolibrary.org/obo/GAZ_00067377">
        <obo:RO_0001025 rdf:resource="http://purl.obolibrary.org/obo/GAZ_00000091"/>
        <oboInOwl:hasOBONamespace>GAZ</oboInOwl:hasOBONamespace>
        <oboInOwl:id>GAZ:00067377</oboInOwl:id>
        <rdfs:label>Coeroeni Ressort</rdfs:label>
    </owl:NamedIndividual>
    


    <!-- http://purl.obolibrary.org/obo/GAZ_00067378 -->

    <owl:NamedIndividual rdf:about="http://purl.obolibrary.org/obo/GAZ_00067378">
        <obo:RO_0001025 rdf:resource="http://purl.obolibrary.org/obo/GAZ_00000091"/>
        <oboInOwl:hasOBONamespace>GAZ</oboInOwl:hasOBONamespace>
        <oboInOwl:id>GAZ:00067378</oboInOwl:id>
        <rdfs:label>Tapanahony Ressort</rdfs:label>
    </owl:NamedIndividual>
    


    <!-- http://purl.obolibrary.org/obo/GAZ_00067379 -->

    <owl:NamedIndividual rdf:about="http://purl.obolibrary.org/obo/GAZ_00067379">
        <obo:RO_0001025 rdf:resource="http://purl.obolibrary.org/obo/GAZ_00000091"/>
        <oboInOwl:hasOBONamespace>GAZ</oboInOwl:hasOBONamespace>
        <oboInOwl:id>GAZ:00067379</oboInOwl:id>
        <rdfs:label>Boven Saramacca Ressort</rdfs:label>
    </owl:NamedIndividual>
    


    <!-- http://purl.obolibrary.org/obo/GAZ_00067380 -->

    <owl:NamedIndividual rdf:about="http://purl.obolibrary.org/obo/GAZ_00067380">
        <obo:RO_0001025 rdf:resource="http://purl.obolibrary.org/obo/GAZ_00000091"/>
        <oboInOwl:hasOBONamespace>GAZ</oboInOwl:hasOBONamespace>
        <oboInOwl:id>GAZ:00067380</oboInOwl:id>
        <rdfs:label>Boven Coppename Ressort</rdfs:label>
    </owl:NamedIndividual>
    


    <!-- http://purl.obolibrary.org/obo/GAZ_00067381 -->

    <owl:NamedIndividual rdf:about="http://purl.obolibrary.org/obo/GAZ_00067381">
        <obo:RO_0001025 rdf:resource="http://purl.obolibrary.org/obo/GAZ_00000091"/>
        <oboInOwl:hasOBONamespace>GAZ</oboInOwl:hasOBONamespace>
        <oboInOwl:id>GAZ:00067381</oboInOwl:id>
        <rdfs:label>Kabalebo Ressort</rdfs:label>
    </owl:NamedIndividual>
    


    <!-- http://purl.obolibrary.org/obo/GAZ_00067382 -->

    <owl:NamedIndividual rdf:about="http://purl.obolibrary.org/obo/GAZ_00067382">
        <obo:RO_0001025 rdf:resource="http://purl.obolibrary.org/obo/GAZ_00000091"/>
        <oboInOwl:hasOBONamespace>GAZ</oboInOwl:hasOBONamespace>
        <oboInOwl:id>GAZ:00067382</oboInOwl:id>
        <rdfs:label>Boven Suriname Ressort</rdfs:label>
    </owl:NamedIndividual>
    


    <!-- http://purl.obolibrary.org/obo/GAZ_00067383 -->

    <owl:NamedIndividual rdf:about="http://purl.obolibrary.org/obo/GAZ_00067383">
        <obo:RO_0001025 rdf:resource="http://purl.obolibrary.org/obo/GAZ_00000082"/>
        <oboInOwl:hasOBONamespace>GAZ</oboInOwl:hasOBONamespace>
        <oboInOwl:id>GAZ:00067383</oboInOwl:id>
        <rdfs:label>Kwatta Ressort</rdfs:label>
    </owl:NamedIndividual>
    


    <!-- http://purl.obolibrary.org/obo/GAZ_00067384 -->

    <owl:NamedIndividual rdf:about="http://purl.obolibrary.org/obo/GAZ_00067384">
        <obo:RO_0001025 rdf:resource="http://purl.obolibrary.org/obo/GAZ_00000082"/>
        <oboInOwl:hasOBONamespace>GAZ</oboInOwl:hasOBONamespace>
        <oboInOwl:id>GAZ:00067384</oboInOwl:id>
        <rdfs:label>Houttuin Ressort</rdfs:label>
    </owl:NamedIndividual>
    


    <!-- http://purl.obolibrary.org/obo/GAZ_00067385 -->

    <owl:NamedIndividual rdf:about="http://purl.obolibrary.org/obo/GAZ_00067385">
        <obo:RO_0001025 rdf:resource="http://purl.obolibrary.org/obo/GAZ_00000082"/>
        <oboInOwl:hasOBONamespace>GAZ</oboInOwl:hasOBONamespace>
        <oboInOwl:id>GAZ:00067385</oboInOwl:id>
        <rdfs:label>Domburg Ressort</rdfs:label>
    </owl:NamedIndividual>
    


    <!-- http://purl.obolibrary.org/obo/GAZ_00067386 -->

    <owl:NamedIndividual rdf:about="http://purl.obolibrary.org/obo/GAZ_00067386">
        <obo:RO_0001025 rdf:resource="http://purl.obolibrary.org/obo/GAZ_00000082"/>
        <oboInOwl:hasOBONamespace>GAZ</oboInOwl:hasOBONamespace>
        <oboInOwl:id>GAZ:00067386</oboInOwl:id>
        <rdfs:label>De Nieuwe Grond Ressort</rdfs:label>
    </owl:NamedIndividual>
    


    <!-- http://purl.obolibrary.org/obo/GAZ_00067387 -->

    <owl:NamedIndividual rdf:about="http://purl.obolibrary.org/obo/GAZ_00067387">
        <obo:RO_0001025 rdf:resource="http://purl.obolibrary.org/obo/GAZ_00000082"/>
        <oboInOwl:hasOBONamespace>GAZ</oboInOwl:hasOBONamespace>
        <oboInOwl:id>GAZ:00067387</oboInOwl:id>
        <rdfs:label>Koewarasan Ressort</rdfs:label>
    </owl:NamedIndividual>
    


    <!-- http://purl.obolibrary.org/obo/GAZ_00067388 -->

    <owl:NamedIndividual rdf:about="http://purl.obolibrary.org/obo/GAZ_00067388">
        <obo:RO_0001025 rdf:resource="http://purl.obolibrary.org/obo/GAZ_00000082"/>
        <oboInOwl:hasOBONamespace>GAZ</oboInOwl:hasOBONamespace>
        <oboInOwl:id>GAZ:00067388</oboInOwl:id>
        <rdfs:label>Saramaccapolder Ressort</rdfs:label>
    </owl:NamedIndividual>
    


    <!-- http://purl.obolibrary.org/obo/GAZ_00082192 -->

    <owl:NamedIndividual rdf:about="http://purl.obolibrary.org/obo/GAZ_00082192">
        <obo:RO_0001025 rdf:resource="http://purl.obolibrary.org/obo/GAZ_00047131"/>
        <obo:IAO_0000115>An island lying off the north coast of Ilha de Marajo in the delta lowlands at the mouth of the Amazon in the State of Para, Brazil.</obo:IAO_0000115>
        <oboInOwl:hasOBONamespace>GAZ</oboInOwl:hasOBONamespace>
        <oboInOwl:id>GAZ:00082192</oboInOwl:id>
        <rdfs:label>Ilha Caviana</rdfs:label>
    </owl:NamedIndividual>
    


    <!-- http://purl.obolibrary.org/obo/GAZ_00082193 -->

    <owl:NamedIndividual rdf:about="http://purl.obolibrary.org/obo/GAZ_00082193">
        <obo:RO_0001025 rdf:resource="http://purl.obolibrary.org/obo/GAZ_00047131"/>
        <obo:IAO_0000115>The second largest island of the River Amazon delta. It lies in the Brazilian State of Para, west of Marajo and near the confluence of the Amazon and the Xingu.</obo:IAO_0000115>
        <oboInOwl:hasOBONamespace>GAZ</oboInOwl:hasOBONamespace>
        <oboInOwl:id>GAZ:00082193</oboInOwl:id>
        <rdfs:label>Ilha Grande do Gurupa</rdfs:label>
    </owl:NamedIndividual>
    


    <!-- http://purl.obolibrary.org/obo/GAZ_00082204 -->

    <owl:NamedIndividual rdf:about="http://purl.obolibrary.org/obo/GAZ_00082204">
        <rdf:type rdf:resource="http://purl.obolibrary.org/obo/ENVO_00000423"/>
        <obo:RO_0001025 rdf:resource="http://purl.obolibrary.org/obo/GAZ_00047130"/>
        <obo:IAO_0000115>A fluvial island. It is bordered by four rivers: Amazon, Madeira, Sucunduri, and Abacaxis. It has been split into four completely separate parts by natural channels just like the one which isolates it from the mainland of America. So it is no longer one island, but indeed four islands. The total area of these islands sums up to 11,850 km2, making Ilha Tupinambarana the largest fluvial group of islands in the world.</obo:IAO_0000115>
        <oboInOwl:hasOBONamespace>GAZ</oboInOwl:hasOBONamespace>
        <oboInOwl:id>GAZ:00082204</oboInOwl:id>
        <rdfs:label>Tupinambarana</rdfs:label>
    </owl:NamedIndividual>
    


    <!-- http://purl.obolibrary.org/obo/GAZ_00082205 -->

    <owl:NamedIndividual rdf:about="http://purl.obolibrary.org/obo/GAZ_00082205">
        <obo:RO_0001025 rdf:resource="http://purl.obolibrary.org/obo/GAZ_00049223"/>
        <obo:IAO_0000115>An archipelago of about 400 fluvial islands.</obo:IAO_0000115>
        <oboInOwl:hasOBONamespace>GAZ</oboInOwl:hasOBONamespace>
        <oboInOwl:id>GAZ:00082205</oboInOwl:id>
        <rdfs:label>Anavilhanas</rdfs:label>
    </owl:NamedIndividual>
    


    <!-- http://purl.obolibrary.org/obo/GAZ_00082206 -->

    <owl:NamedIndividual rdf:about="http://purl.obolibrary.org/obo/GAZ_00082206">
        <obo:RO_0001025 rdf:resource="http://purl.obolibrary.org/obo/GAZ_00082205"/>
        <oboInOwl:hasOBONamespace>GAZ</oboInOwl:hasOBONamespace>
        <oboInOwl:id>GAZ:00082206</oboInOwl:id>
        <rdfs:label>Estacao Ecologica Anavilhanas</rdfs:label>
    </owl:NamedIndividual>
    


    <!-- http://purl.obolibrary.org/obo/GAZ_00095459 -->

    <owl:NamedIndividual rdf:about="http://purl.obolibrary.org/obo/GAZ_00095459">
        <obo:IAO_0000115>A national park. Situa-se na Floresta Amazonica, nos municipios de Pedra Branca, Serra do Navio, Laranjal do Jari, Oiapoque e Calcoene, nos estados do Amapa e Para, Brasil.</obo:IAO_0000115>
        <oboInOwl:hasOBONamespace>GAZ</oboInOwl:hasOBONamespace>
        <oboInOwl:id>GAZ:00095459</oboInOwl:id>
        <rdfs:label>Parque Nacional das Montanhas do Tumucumaque</rdfs:label>
    </owl:NamedIndividual>
    


    <!-- http://purl.obolibrary.org/obo/GAZ_00120745 -->

    <owl:NamedIndividual rdf:about="http://purl.obolibrary.org/obo/GAZ_00120745">
        <obo:RO_0001025 rdf:resource="http://purl.obolibrary.org/obo/GAZ_00120746"/>
        <obo:IAO_0000115>Una isla fluvial boliviana situada al este del departamento del Beni en las coordenadas, en la frontera con Brasil, la isla se encuentra completamente rodeada por el rio Itenez.</obo:IAO_0000115>
        <oboInOwl:hasOBONamespace>GAZ</oboInOwl:hasOBONamespace>
        <oboInOwl:id>GAZ:00120745</oboInOwl:id>
        <rdfs:label>Isla Cumprida</rdfs:label>
    </owl:NamedIndividual>
    


    <!-- http://purl.obolibrary.org/obo/GAZ_00120746 -->

    <owl:NamedIndividual rdf:about="http://purl.obolibrary.org/obo/GAZ_00120746">
        <obo:IAO_0000115>Un rio boliviano - brasileno, perteneciente a la cuenca del amazonas, nace en Brasil donde recorre en direccion nor-oeste unos 560 kilometros en territorio brasileno hasta uno de sus afluente llamado rio Verde donde pasa a formar una frontera natural entre los dos paises de 970 kilometros hasta su desembocadura en el rio Mamore.</obo:IAO_0000115>
        <oboInOwl:hasOBONamespace>GAZ</oboInOwl:hasOBONamespace>
        <oboInOwl:id>GAZ:00120746</oboInOwl:id>
        <rdfs:label>Rio Itenez</rdfs:label>
    </owl:NamedIndividual>
    


    <!-- http://purl.obolibrary.org/obo/GAZ_00120747 -->

    <owl:NamedIndividual rdf:about="http://purl.obolibrary.org/obo/GAZ_00120747">
        <obo:IAO_0000115>Un rio amazonico boliviano-brasilero, aunque la mayor parte de su recorrido lo hace en territorio boliviano siendo este el mas importante del pais, pertenece a la cuenca del Amazonas, nace de las confluencias de los rios Chapare y Mamorecillo en las coordenadas entre los departamentos de Santa Cruz y Cochabamba, a 24 kilometros al sur de la desembocadura de uno de sus grandes afluentes el rio Grande, el rio discurre en direccion norte en todo su recorrido, aunque el algunas zonas discurre en direccion noroeste y noreste.</obo:IAO_0000115>
        <oboInOwl:hasOBONamespace>GAZ</oboInOwl:hasOBONamespace>
        <oboInOwl:id>GAZ:00120747</oboInOwl:id>
        <rdfs:label>Rio Mamore</rdfs:label>
    </owl:NamedIndividual>
    


    <!-- http://purl.obolibrary.org/obo/GAZ_00120748 -->

    <owl:NamedIndividual rdf:about="http://purl.obolibrary.org/obo/GAZ_00120748">
        <obo:RO_0001025 rdf:resource="http://purl.obolibrary.org/obo/GAZ_00120747"/>
        <obo:IAO_0000115>Una isla fluvial amazonica ubicada sobre el rio Mamore. La soberania sobre la isla esta en disputa pasiva entre Brasil y Bolivia. Para Bolivia la isla forma parte del Departamento del Beni y para Brasil es parte del Municipio de Guajara-Mirim en el estado de Rondonia.</obo:IAO_0000115>
        <oboInOwl:hasOBONamespace>GAZ</oboInOwl:hasOBONamespace>
        <oboInOwl:id>GAZ:00120748</oboInOwl:id>
        <rdfs:label>Isla Suarez</rdfs:label>
    </owl:NamedIndividual>
    


    <!-- http://purl.obolibrary.org/obo/GAZ_00246888 -->

    <owl:NamedIndividual rdf:about="http://purl.obolibrary.org/obo/GAZ_00246888">
        <obo:IAO_0000115>A group of 6 lakes in the highlands of the upper Rio Negro of Brazil.</obo:IAO_0000115>
        <oboInOwl:hasOBONamespace>GAZ</oboInOwl:hasOBONamespace>
        <oboInOwl:id>GAZ:00246888</oboInOwl:id>
        <rdfs:label>Morro de 6 Lagos</rdfs:label>
    </owl:NamedIndividual>
    


    <!-- http://purl.obolibrary.org/obo/GAZ_00246921 -->

    <owl:NamedIndividual rdf:about="http://purl.obolibrary.org/obo/GAZ_00246921">
        <obo:RO_0001025 rdf:resource="http://purl.obolibrary.org/obo/GAZ_00047131"/>
        <obo:IAO_0000115>An island.</obo:IAO_0000115>
        <oboInOwl:hasOBONamespace>GAZ</oboInOwl:hasOBONamespace>
        <oboInOwl:id>GAZ:00246921</oboInOwl:id>
        <rdfs:label>Ilha do Brique</rdfs:label>
    </owl:NamedIndividual>
    


    <!-- http://purl.obolibrary.org/obo/GAZ_00246922 -->

    <owl:NamedIndividual rdf:about="http://purl.obolibrary.org/obo/GAZ_00246922">
        <obo:RO_0001025 rdf:resource="http://purl.obolibrary.org/obo/GAZ_00047131"/>
        <obo:IAO_0000115>An island.</obo:IAO_0000115>
        <oboInOwl:hasOBONamespace>GAZ</oboInOwl:hasOBONamespace>
        <oboInOwl:id>GAZ:00246922</oboInOwl:id>
        <rdfs:label>Ilha Janauco</rdfs:label>
    </owl:NamedIndividual>
    


    <!-- http://purl.obolibrary.org/obo/GAZ_00246923 -->

    <owl:NamedIndividual rdf:about="http://purl.obolibrary.org/obo/GAZ_00246923">
        <obo:RO_0001025 rdf:resource="http://purl.obolibrary.org/obo/GAZ_00047131"/>
        <obo:IAO_0000115>An island.</obo:IAO_0000115>
        <oboInOwl:hasOBONamespace>GAZ</oboInOwl:hasOBONamespace>
        <oboInOwl:id>GAZ:00246923</oboInOwl:id>
        <rdfs:label>Ilha Mexiana</rdfs:label>
    </owl:NamedIndividual>
    


    <!-- http://purl.obolibrary.org/obo/GAZ_00246935 -->

    <owl:NamedIndividual rdf:about="http://purl.obolibrary.org/obo/GAZ_00246935">
        <obo:RO_0001025 rdf:resource="http://purl.obolibrary.org/obo/GAZ_00047131"/>
        <obo:IAO_0000115>A sea bay.</obo:IAO_0000115>
        <oboInOwl:hasOBONamespace>GAZ</oboInOwl:hasOBONamespace>
        <oboInOwl:id>GAZ:00246935</oboInOwl:id>
        <rdfs:label>Baia de Marajo</rdfs:label>
    </owl:NamedIndividual>
    


    <!-- http://purl.obolibrary.org/obo/GAZ_00246936 -->

    <owl:NamedIndividual rdf:about="http://purl.obolibrary.org/obo/GAZ_00246936">
        <obo:RO_0001025 rdf:resource="http://purl.obolibrary.org/obo/GAZ_00047132"/>
        <obo:IAO_0000115>A brackish lake.</obo:IAO_0000115>
        <oboInOwl:hasOBONamespace>GAZ</oboInOwl:hasOBONamespace>
        <oboInOwl:id>GAZ:00246936</oboInOwl:id>
        <rdfs:label>Lago Arari</rdfs:label>
    </owl:NamedIndividual>
    


    <!-- http://purl.obolibrary.org/obo/GAZ_00254087 -->

    <owl:NamedIndividual rdf:about="http://purl.obolibrary.org/obo/GAZ_00254087">
        <obo:RO_0001025 rdf:resource="http://purl.obolibrary.org/obo/GAZ_00047130"/>
        <obo:IAO_0000115>A river that rises north of Lake Titicaca, in the Arequipa region of South America.</obo:IAO_0000115>
        <oboInOwl:hasOBONamespace>GAZ</oboInOwl:hasOBONamespace>
        <oboInOwl:id>GAZ:00254087</oboInOwl:id>
        <rdfs:label>Rio Ucayali</rdfs:label>
    </owl:NamedIndividual>
    


    <!-- http://purl.obolibrary.org/obo/GAZ_00256487 -->

    <owl:NamedIndividual rdf:about="http://purl.obolibrary.org/obo/GAZ_00256487">
        <obo:RO_0001025 rdf:resource="http://purl.obolibrary.org/obo/GAZ_00000088"/>
        <obo:IAO_0000115>A lake.</obo:IAO_0000115>
        <oboInOwl:hasOBONamespace>GAZ</oboInOwl:hasOBONamespace>
        <oboInOwl:id>GAZ:00256487</oboInOwl:id>
        <rdfs:label>Bigi Pan</rdfs:label>
    </owl:NamedIndividual>
    


    <!-- http://purl.obolibrary.org/obo/GAZ_00256488 -->

    <owl:NamedIndividual rdf:about="http://purl.obolibrary.org/obo/GAZ_00256488">
        <obo:RO_0001025 rdf:resource="http://purl.obolibrary.org/obo/GAZ_00000088"/>
        <obo:IAO_0000115>A wetland.</obo:IAO_0000115>
        <oboInOwl:hasOBONamespace>GAZ</oboInOwl:hasOBONamespace>
        <oboInOwl:id>GAZ:00256488</oboInOwl:id>
        <rdfs:label>Wageningen Swamp</rdfs:label>
    </owl:NamedIndividual>
    


    <!-- http://purl.obolibrary.org/obo/GAZ_00256490 -->

    <owl:NamedIndividual rdf:about="http://purl.obolibrary.org/obo/GAZ_00256490">
        <obo:RO_0001025 rdf:resource="http://purl.obolibrary.org/obo/GAZ_00000091"/>
        <obo:IAO_0000115>A headwater of the Coppename River. It has its sources in the western and central parts of the north side of the Wilhelmina mountains and from the south east region of the Bakhuys Mountains.</obo:IAO_0000115>
        <oboInOwl:hasOBONamespace>GAZ</oboInOwl:hasOBONamespace>
        <oboInOwl:id>GAZ:00256490</oboInOwl:id>
        <rdfs:label>Middle Coppename River</rdfs:label>
    </owl:NamedIndividual>
    


    <!-- http://purl.obolibrary.org/obo/GAZ_00256491 -->

    <owl:NamedIndividual rdf:about="http://purl.obolibrary.org/obo/GAZ_00256491">
        <obo:RO_0001025 rdf:resource="http://purl.obolibrary.org/obo/GAZ_00000091"/>
        <obo:IAO_0000115>A headwater of the Coppename River.</obo:IAO_0000115>
        <oboInOwl:hasOBONamespace>GAZ</oboInOwl:hasOBONamespace>
        <oboInOwl:id>GAZ:00256491</oboInOwl:id>
        <rdfs:label>Left Coppename River</rdfs:label>
    </owl:NamedIndividual>
    


    <!-- http://purl.obolibrary.org/obo/GAZ_00256492 -->

    <owl:NamedIndividual rdf:about="http://purl.obolibrary.org/obo/GAZ_00256492">
        <obo:RO_0001025 rdf:resource="http://purl.obolibrary.org/obo/GAZ_00000091"/>
        <obo:IAO_0000115>A headwater of the Coppename River. It originates on the northeast slope of the Wilhelmina range, Tafelberg, and the western parts of the Emmakette.</obo:IAO_0000115>
        <oboInOwl:hasOBONamespace>GAZ</oboInOwl:hasOBONamespace>
        <oboInOwl:id>GAZ:00256492</oboInOwl:id>
        <rdfs:label>Right Midden Coppename River</rdfs:label>
    </owl:NamedIndividual>
    


    <!-- http://purl.obolibrary.org/obo/GAZ_00256499 -->

    <owl:NamedIndividual rdf:about="http://purl.obolibrary.org/obo/GAZ_00256499">
        <obo:RO_0001025 rdf:resource="http://purl.obolibrary.org/obo/GAZ_00067348"/>
        <obo:IAO_0000115>A populated place. The second largest city in Suriname. It is the capital city of the Nickerie district. Nieuw Nickerie lies on the mouth of the Nickerie river on the Atlantic coast, opposite the mouth of the Corantijn river (Courantyne) and the Guyanese town of Corriverton (Springlands).</obo:IAO_0000115>
        <oboInOwl:hasOBONamespace>GAZ</oboInOwl:hasOBONamespace>
        <oboInOwl:id>GAZ:00256499</oboInOwl:id>
        <rdfs:label>Nieuw Nickerie</rdfs:label>
    </owl:NamedIndividual>
    


    <!-- http://purl.obolibrary.org/obo/GAZ_00256501 -->

    <owl:NamedIndividual rdf:about="http://purl.obolibrary.org/obo/GAZ_00256501">
        <obo:RO_0001025 rdf:resource="http://purl.obolibrary.org/obo/GAZ_00000091"/>
        <obo:IAO_0000115>A river of Suriname.</obo:IAO_0000115>
        <oboInOwl:hasOBONamespace>GAZ</oboInOwl:hasOBONamespace>
        <oboInOwl:id>GAZ:00256501</oboInOwl:id>
        <rdfs:label>Kabalebo River</rdfs:label>
    </owl:NamedIndividual>
    


    <!-- http://purl.obolibrary.org/obo/GAZ_00256502 -->

    <owl:NamedIndividual rdf:about="http://purl.obolibrary.org/obo/GAZ_00256502">
        <obo:RO_0001025 rdf:resource="http://purl.obolibrary.org/obo/GAZ_00000091"/>
        <obo:IAO_0000115>A river of Suriname.</obo:IAO_0000115>
        <oboInOwl:hasOBONamespace>GAZ</oboInOwl:hasOBONamespace>
        <oboInOwl:id>GAZ:00256502</oboInOwl:id>
        <rdfs:label>Lucie River</rdfs:label>
    </owl:NamedIndividual>
    


    <!-- http://purl.obolibrary.org/obo/GAZ_00256503 -->

    <owl:NamedIndividual rdf:about="http://purl.obolibrary.org/obo/GAZ_00256503">
        <obo:RO_0001025 rdf:resource="http://purl.obolibrary.org/obo/GAZ_00002525"/>
        <obo:IAO_0000115>A river of Suriname.</obo:IAO_0000115>
        <oboInOwl:hasOBONamespace>GAZ</oboInOwl:hasOBONamespace>
        <oboInOwl:id>GAZ:00256503</oboInOwl:id>
        <rdfs:label>Sipaliwini River</rdfs:label>
    </owl:NamedIndividual>
    


    <!-- http://purl.obolibrary.org/obo/GAZ_00256506 -->

    <owl:NamedIndividual rdf:about="http://purl.obolibrary.org/obo/GAZ_00256506">
        <obo:RO_0001025 rdf:resource="http://purl.obolibrary.org/obo/GAZ_00005324"/>
    </owl:NamedIndividual>
    


    <!-- http://purl.obolibrary.org/obo/GAZ_00256507 -->

    <owl:NamedIndividual rdf:about="http://purl.obolibrary.org/obo/GAZ_00256507">
        <rdf:type rdf:resource="http://purl.obolibrary.org/obo/ENVO_00000856"/>
        <obo:RO_0001025 rdf:resource="http://purl.obolibrary.org/obo/GAZ_00067331"/>
        <obo:IAO_0000115>A populated place. A town in Suriname, located on the eastern bank of the Suriname River, directly opposite the capital Paramaribo.</obo:IAO_0000115>
        <oboInOwl:hasOBONamespace>GAZ</oboInOwl:hasOBONamespace>
        <oboInOwl:id>GAZ:00256507</oboInOwl:id>
        <rdfs:label>Meerzorg</rdfs:label>
    </owl:NamedIndividual>
    


    <!-- http://purl.obolibrary.org/obo/GAZ_00256508 -->

    <owl:NamedIndividual rdf:about="http://purl.obolibrary.org/obo/GAZ_00256508">
        <obo:RO_0001025 rdf:resource="http://purl.obolibrary.org/obo/GAZ_00067328"/>
        <obo:IAO_0000115>A populated place. The capital of the Commewijne District in Suriname. It is a small coastal town situated near the mouth of the Suriname River just across from Paramaribo.</obo:IAO_0000115>
        <oboInOwl:hasOBONamespace>GAZ</oboInOwl:hasOBONamespace>
        <oboInOwl:id>GAZ:00256508</oboInOwl:id>
        <rdfs:label>Nieuw Amsterdam</rdfs:label>
    </owl:NamedIndividual>
    


    <!-- http://purl.obolibrary.org/obo/GAZ_00256509 -->

    <owl:NamedIndividual rdf:about="http://purl.obolibrary.org/obo/GAZ_00256509">
        <obo:RO_0001025 rdf:resource="http://purl.obolibrary.org/obo/GAZ_00000085"/>
        <obo:IAO_0000115>A river in northern Suriname.</obo:IAO_0000115>
        <oboInOwl:hasOBONamespace>GAZ</oboInOwl:hasOBONamespace>
        <oboInOwl:id>GAZ:00256509</oboInOwl:id>
        <rdfs:label>Commewijne River</rdfs:label>
    </owl:NamedIndividual>
    


    <!-- http://purl.obolibrary.org/obo/GAZ_00256512 -->

    <owl:NamedIndividual rdf:about="http://purl.obolibrary.org/obo/GAZ_00256512">
        <rdf:type rdf:resource="http://purl.obolibrary.org/obo/ENVO_00000856"/>
        <obo:RO_0001025 rdf:resource="http://purl.obolibrary.org/obo/GAZ_00067342"/>
        <obo:IAO_0000115>A populated place. A town in eastern Suriname, and is capital of the Marowijne District. The town lies on the west bank of the Marowijne River.</obo:IAO_0000115>
        <oboInOwl:hasOBONamespace>GAZ</oboInOwl:hasOBONamespace>
        <oboInOwl:id>GAZ:00256512</oboInOwl:id>
        <rdfs:label>Albina</rdfs:label>
    </owl:NamedIndividual>
    


    <!-- http://purl.obolibrary.org/obo/GAZ_00256514 -->

    <owl:NamedIndividual rdf:about="http://purl.obolibrary.org/obo/GAZ_00256514">
        <obo:RO_0001025 rdf:resource="http://purl.obolibrary.org/obo/GAZ_00000091"/>
        <obo:IAO_0000115>A river.</obo:IAO_0000115>
        <oboInOwl:hasOBONamespace>GAZ</oboInOwl:hasOBONamespace>
        <oboInOwl:id>GAZ:00256514</oboInOwl:id>
        <rdfs:label>Oelemari River</rdfs:label>
    </owl:NamedIndividual>
    


    <!-- http://purl.obolibrary.org/obo/GAZ_00256515 -->

    <owl:NamedIndividual rdf:about="http://purl.obolibrary.org/obo/GAZ_00256515">
        <obo:RO_0001025 rdf:resource="http://purl.obolibrary.org/obo/GAZ_00002525"/>
        <obo:IAO_0000115>A river in Suriname.</obo:IAO_0000115>
        <oboInOwl:hasOBONamespace>GAZ</oboInOwl:hasOBONamespace>
        <oboInOwl:id>GAZ:00256515</oboInOwl:id>
        <rdfs:label>Gonini River</rdfs:label>
    </owl:NamedIndividual>
    


    <!-- http://purl.obolibrary.org/obo/GAZ_00256516 -->

    <owl:NamedIndividual rdf:about="http://purl.obolibrary.org/obo/GAZ_00256516">
        <obo:RO_0001025 rdf:resource="http://purl.obolibrary.org/obo/GAZ_00000091"/>
        <obo:IAO_0000115>A river in the south eastern part of Suriname, South America. It joins the Marowijne River at Stoelmans Island.</obo:IAO_0000115>
        <oboInOwl:hasOBONamespace>GAZ</oboInOwl:hasOBONamespace>
        <oboInOwl:id>GAZ:00256516</oboInOwl:id>
        <rdfs:label>Tapanahony River</rdfs:label>
    </owl:NamedIndividual>
    


    <!-- http://purl.obolibrary.org/obo/GAZ_00256517 -->

    <owl:NamedIndividual rdf:about="http://purl.obolibrary.org/obo/GAZ_00256517">
        <obo:RO_0001025 rdf:resource="http://purl.obolibrary.org/obo/GAZ_00000091"/>
        <obo:IAO_0000115>A river of Suriname.</obo:IAO_0000115>
        <oboInOwl:hasOBONamespace>GAZ</oboInOwl:hasOBONamespace>
        <oboInOwl:id>GAZ:00256517</oboInOwl:id>
        <rdfs:label>Paloemeu River</rdfs:label>
    </owl:NamedIndividual>
    


    <!-- http://purl.obolibrary.org/obo/GAZ_00256518 -->

    <owl:NamedIndividual rdf:about="http://purl.obolibrary.org/obo/GAZ_00256518">
        <obo:RO_0001025 rdf:resource="http://purl.obolibrary.org/obo/GAZ_00000088"/>
        <obo:IAO_0000115>A protected area. Established 1972.</obo:IAO_0000115>
        <oboInOwl:hasOBONamespace>GAZ</oboInOwl:hasOBONamespace>
        <oboInOwl:id>GAZ:00256518</oboInOwl:id>
        <rdfs:label>Hertenrits Nature Reserve</rdfs:label>
    </owl:NamedIndividual>
    


    <!-- http://purl.obolibrary.org/obo/GAZ_00256519 -->

    <owl:NamedIndividual rdf:about="http://purl.obolibrary.org/obo/GAZ_00256519">
        <obo:RO_0001025 rdf:resource="http://purl.obolibrary.org/obo/GAZ_00000087"/>
        <obo:IAO_0000115>A protected area. Established 1960.</obo:IAO_0000115>
        <oboInOwl:hasOBONamespace>GAZ</oboInOwl:hasOBONamespace>
        <oboInOwl:id>GAZ:00256519</oboInOwl:id>
        <rdfs:label>Galibi Nature Reserve</rdfs:label>
    </owl:NamedIndividual>
    


    <!-- http://purl.obolibrary.org/obo/GAZ_00256520 -->

    <owl:NamedIndividual rdf:about="http://purl.obolibrary.org/obo/GAZ_00256520">
        <obo:RO_0001025 rdf:resource="http://purl.obolibrary.org/obo/GAZ_00000087"/>
        <obo:IAO_0000115>A protected area. Established 1966.</obo:IAO_0000115>
        <oboInOwl:hasOBONamespace>GAZ</oboInOwl:hasOBONamespace>
        <oboInOwl:id>GAZ:00256520</oboInOwl:id>
        <rdfs:label>Wia Wia Nature Reserve</rdfs:label>
    </owl:NamedIndividual>
    


    <!-- http://purl.obolibrary.org/obo/GAZ_00256521 -->

    <owl:NamedIndividual rdf:about="http://purl.obolibrary.org/obo/GAZ_00256521">
        <obo:RO_0001025 rdf:resource="http://purl.obolibrary.org/obo/GAZ_00000090"/>
        <obo:IAO_0000115>A protected area. Established 1966.</obo:IAO_0000115>
        <oboInOwl:hasOBONamespace>GAZ</oboInOwl:hasOBONamespace>
        <oboInOwl:id>GAZ:00256521</oboInOwl:id>
        <rdfs:label>Coppename Nature Reserve</rdfs:label>
    </owl:NamedIndividual>
    


    <!-- http://purl.obolibrary.org/obo/GAZ_00256522 -->

    <owl:NamedIndividual rdf:about="http://purl.obolibrary.org/obo/GAZ_00256522">
        <obo:RO_0001025 rdf:resource="http://purl.obolibrary.org/obo/GAZ_00000086"/>
        <obo:IAO_0000115>A protected area. Established 1986.</obo:IAO_0000115>
        <oboInOwl:hasOBONamespace>GAZ</oboInOwl:hasOBONamespace>
        <oboInOwl:id>GAZ:00256522</oboInOwl:id>
        <rdfs:label>Peruvia Nature Reserve</rdfs:label>
    </owl:NamedIndividual>
    


    <!-- http://purl.obolibrary.org/obo/GAZ_00256523 -->

    <owl:NamedIndividual rdf:about="http://purl.obolibrary.org/obo/GAZ_00256523">
        <obo:RO_0001025 rdf:resource="http://purl.obolibrary.org/obo/GAZ_00000087"/>
        <obo:IAO_0000115>A protected area. Established 1986.</obo:IAO_0000115>
        <oboInOwl:hasOBONamespace>GAZ</oboInOwl:hasOBONamespace>
        <oboInOwl:id>GAZ:00256523</oboInOwl:id>
        <rdfs:label>Wanekreek Nature Reserve</rdfs:label>
    </owl:NamedIndividual>
    


    <!-- http://purl.obolibrary.org/obo/GAZ_00256524 -->

    <owl:NamedIndividual rdf:about="http://purl.obolibrary.org/obo/GAZ_00256524">
        <obo:RO_0001025 rdf:resource="http://purl.obolibrary.org/obo/GAZ_00000089"/>
        <obo:IAO_0000115>A protected area.</obo:IAO_0000115>
        <oboInOwl:hasOBONamespace>GAZ</oboInOwl:hasOBONamespace>
        <oboInOwl:id>GAZ:00256524</oboInOwl:id>
        <rdfs:label>Copi Nature Reserve</rdfs:label>
    </owl:NamedIndividual>
    


    <!-- http://purl.obolibrary.org/obo/GAZ_00256525 -->

    <owl:NamedIndividual rdf:about="http://purl.obolibrary.org/obo/GAZ_00256525">
        <obo:RO_0001025 rdf:resource="http://purl.obolibrary.org/obo/GAZ_00000089"/>
        <obo:IAO_0000115>A protected area.</obo:IAO_0000115>
        <oboInOwl:hasOBONamespace>GAZ</oboInOwl:hasOBONamespace>
        <oboInOwl:id>GAZ:00256525</oboInOwl:id>
        <rdfs:label>Boven Coesewijne Nature Reserve</rdfs:label>
    </owl:NamedIndividual>
    


    <!-- http://purl.obolibrary.org/obo/GAZ_00256526 -->

    <owl:NamedIndividual rdf:about="http://purl.obolibrary.org/obo/GAZ_00256526">
        <obo:RO_0001025 rdf:resource="http://purl.obolibrary.org/obo/GAZ_00000084"/>
        <obo:IAO_0000115>A protected area. Established 1966.</obo:IAO_0000115>
        <oboInOwl:hasOBONamespace>GAZ</oboInOwl:hasOBONamespace>
        <oboInOwl:id>GAZ:00256526</oboInOwl:id>
        <rdfs:label>Brinckheuvel Nature Reserve</rdfs:label>
    </owl:NamedIndividual>
    


    <!-- http://purl.obolibrary.org/obo/GAZ_00256527 -->

    <owl:NamedIndividual rdf:about="http://purl.obolibrary.org/obo/GAZ_00256527">
        <obo:RO_0001025 rdf:resource="http://purl.obolibrary.org/obo/GAZ_00000091"/>
        <obo:IAO_0000115>A protected area. Established 1972.</obo:IAO_0000115>
        <oboInOwl:hasOBONamespace>GAZ</oboInOwl:hasOBONamespace>
        <oboInOwl:id>GAZ:00256527</oboInOwl:id>
        <rdfs:label>Sipaliwini Nature Reserve</rdfs:label>
    </owl:NamedIndividual>
    


    <!-- http://purl.obolibrary.org/obo/GAZ_00256528 -->

    <owl:NamedIndividual rdf:about="http://purl.obolibrary.org/obo/GAZ_00256528">
        <obo:RO_0001025 rdf:resource="http://purl.obolibrary.org/obo/GAZ_00000084"/>
        <obo:IAO_0000115>A protected area. Established 1972; enlarged 2002.</obo:IAO_0000115>
        <oboInOwl:hasOBONamespace>GAZ</oboInOwl:hasOBONamespace>
        <oboInOwl:id>GAZ:00256528</oboInOwl:id>
        <rdfs:label>Brownsberg Nature Park</rdfs:label>
    </owl:NamedIndividual>
    


    <!-- http://purl.obolibrary.org/obo/GAZ_00256529 -->

    <owl:NamedIndividual rdf:about="http://purl.obolibrary.org/obo/GAZ_00256529">
        <obo:RO_0001025 rdf:resource="http://purl.obolibrary.org/obo/GAZ_00056742"/>
        <obo:IAO_0000115>A region of the Central Suriname Nature Reserve. Was, formerly, a separate protected area.</obo:IAO_0000115>
        <oboInOwl:hasOBONamespace>GAZ</oboInOwl:hasOBONamespace>
        <oboInOwl:id>GAZ:00256529</oboInOwl:id>
        <rdfs:label>Raleighvallen Area, Central Suriname Nature Reserve</rdfs:label>
    </owl:NamedIndividual>
    


    <!-- http://purl.obolibrary.org/obo/GAZ_00256530 -->

    <owl:NamedIndividual rdf:about="http://purl.obolibrary.org/obo/GAZ_00256530">
        <obo:RO_0001025 rdf:resource="http://purl.obolibrary.org/obo/GAZ_00056742"/>
        <obo:IAO_0000115>A region of the Central Suriname Nature Reserve. Was, formerly, a separate protected area.</obo:IAO_0000115>
        <oboInOwl:hasOBONamespace>GAZ</oboInOwl:hasOBONamespace>
        <oboInOwl:id>GAZ:00256530</oboInOwl:id>
        <rdfs:label>Tafelberg Area, Central Suriname Nature Reserve</rdfs:label>
    </owl:NamedIndividual>
    


    <!-- http://purl.obolibrary.org/obo/GAZ_00256531 -->

    <owl:NamedIndividual rdf:about="http://purl.obolibrary.org/obo/GAZ_00256531">
        <obo:RO_0001025 rdf:resource="http://purl.obolibrary.org/obo/GAZ_00056742"/>
        <obo:IAO_0000115>A region of the Central Suriname Nature Reserve. Was, formerly, a separate protected area.</obo:IAO_0000115>
        <oboInOwl:hasOBONamespace>GAZ</oboInOwl:hasOBONamespace>
        <oboInOwl:id>GAZ:00256531</oboInOwl:id>
        <rdfs:label>Eilerts de Haan Area, Central Suriname Nature Reserve</rdfs:label>
    </owl:NamedIndividual>
    


    <!-- http://purl.obolibrary.org/obo/GAZ_00256532 -->

    <owl:NamedIndividual rdf:about="http://purl.obolibrary.org/obo/GAZ_00256532">
        <obo:RO_0001025 rdf:resource="http://purl.obolibrary.org/obo/GAZ_00000088"/>
        <obo:IAO_0000115>A wetland. Includes alluvial plains between the Courantyne and Maratakka Rivers, S of the Nickerie rice growing area.</obo:IAO_0000115>
        <oboInOwl:hasOBONamespace>GAZ</oboInOwl:hasOBONamespace>
        <oboInOwl:id>GAZ:00256532</oboInOwl:id>
        <rdfs:label>Nanni Swamp</rdfs:label>
    </owl:NamedIndividual>
    


    <!-- http://purl.obolibrary.org/obo/GAZ_00256533 -->

    <owl:NamedIndividual rdf:about="http://purl.obolibrary.org/obo/GAZ_00256533">
        <obo:RO_0001025 rdf:resource="http://purl.obolibrary.org/obo/GAZ_00067347"/>
        <obo:IAO_0000115>A river.</obo:IAO_0000115>
        <oboInOwl:hasOBONamespace>GAZ</oboInOwl:hasOBONamespace>
        <oboInOwl:id>GAZ:00256533</oboInOwl:id>
        <rdfs:label>Maratakka River</rdfs:label>
    </owl:NamedIndividual>
    


    <!-- http://purl.obolibrary.org/obo/GAZ_00256535 -->

    <owl:NamedIndividual rdf:about="http://purl.obolibrary.org/obo/GAZ_00256535">
        <obo:RO_0001025 rdf:resource="http://purl.obolibrary.org/obo/GAZ_00000088"/>
        <obo:IAO_0000115>A wetland. An open savanna with several rivers and some permanent freshwater marshes and seasonally flooded grasslands. Located on the Brazil border.</obo:IAO_0000115>
        <oboInOwl:hasOBONamespace>GAZ</oboInOwl:hasOBONamespace>
        <oboInOwl:id>GAZ:00256535</oboInOwl:id>
        <rdfs:label>Sipallwini Savanna</rdfs:label>
    </owl:NamedIndividual>
    


    <!-- 
    ///////////////////////////////////////////////////////////////////////////////////////
    //
    // Annotations
    //
    ///////////////////////////////////////////////////////////////////////////////////////
     -->

    <rdf:Description rdf:about="http://purl.obolibrary.org/obo/GAZ_00000082">
        <rdfs:label>Wanica District</rdfs:label>
        <oboInOwl:hasOBONamespace>GAZ</oboInOwl:hasOBONamespace>
        <obo:IAO_0000115>A district of Suriname, in the northeast. Wanica&apos;s capital city is Lelydorp.</obo:IAO_0000115>
        <oboInOwl:id>GAZ:00000082</oboInOwl:id>
    </rdf:Description>
    <rdf:Description rdf:about="http://purl.obolibrary.org/obo/GAZ_00000083">
        <rdfs:label>Lelydorp</rdfs:label>
        <oboInOwl:hasOBONamespace>GAZ</oboInOwl:hasOBONamespace>
        <oboInOwl:id>GAZ:00000083</oboInOwl:id>
    </rdf:Description>
    <rdf:Description rdf:about="http://purl.obolibrary.org/obo/GAZ_00000084">
        <oboInOwl:hasOBONamespace>GAZ</oboInOwl:hasOBONamespace>
        <oboInOwl:id>GAZ:00000084</oboInOwl:id>
        <obo:IAO_0000115>A district of Suriname. Its capital city is Brokopondo; other towns include Brownsweg and Kwakoegron.</obo:IAO_0000115>
        <rdfs:label>Brokopondo District</rdfs:label>
    </rdf:Description>
    <rdf:Description rdf:about="http://purl.obolibrary.org/obo/GAZ_00000085">
        <oboInOwl:hasOBONamespace>GAZ</oboInOwl:hasOBONamespace>
        <rdfs:label>Commewijne District</rdfs:label>
        <oboInOwl:id>GAZ:00000085</oboInOwl:id>
        <obo:IAO_0000115>A district of Suriname, located on the right bank of the Suriname River. Commewijne&apos;s capital city is Nieuw Amsterdam. Alliance is another major town.</obo:IAO_0000115>
    </rdf:Description>
    <rdf:Description rdf:about="http://purl.obolibrary.org/obo/GAZ_00000086">
        <oboInOwl:hasOBONamespace>GAZ</oboInOwl:hasOBONamespace>
        <obo:IAO_0000115>A district of Suriname, situated on the coast. Coronie&apos;s capital city is Totness, with other towns including Corneliskondre, Friendship, Jenny. The district border the Atlantic Ocean to the north, the Surinamese district of Saramacca to the east, the Surinamese district of Sipaliwini to the south and the Surinamese district of Nickerie to the west.</obo:IAO_0000115>
        <oboInOwl:id>GAZ:00000086</oboInOwl:id>
        <rdfs:label>Coronie District</rdfs:label>
    </rdf:Description>
    <rdf:Description rdf:about="http://purl.obolibrary.org/obo/GAZ_00000087">
        <obo:IAO_0000115>A district of Suriname, located on the north-east coast. Marowijne&apos;s capital city is Albina, with other towns including Moengo and Wanhatti. The district borders the Atlantic Ocean to the north, French Guiana to the east, the Surinamese district of Sipaliwini to the south and the Surinamese districts of Commewijne and Para to the west.</obo:IAO_0000115>
        <oboInOwl:hasOBONamespace>GAZ</oboInOwl:hasOBONamespace>
        <rdfs:label>Marowijne District</rdfs:label>
        <oboInOwl:id>GAZ:00000087</oboInOwl:id>
    </rdf:Description>
    <rdf:Description rdf:about="http://purl.obolibrary.org/obo/GAZ_00000088">
        <oboInOwl:hasOBONamespace>GAZ</oboInOwl:hasOBONamespace>
        <rdfs:label>Nickerie District</rdfs:label>
        <obo:IAO_0000115>A district of Suriname, on the north-west coast. Nickerie&apos;s capital city is Nieuw-Nickerie, the second largest city in the country. Other towns include Washoda and Wageningen. The district borders the Atlantic Ocean to the north, the Surinamese district of Coronie to the east, the Surinamese district of Sipaliwini to the south and Guyana to the west.</obo:IAO_0000115>
        <oboInOwl:id>GAZ:00000088</oboInOwl:id>
    </rdf:Description>
    <rdf:Description rdf:about="http://purl.obolibrary.org/obo/GAZ_00000089">
        <obo:IAO_0000115>A district of Suriname, in the north. Para&apos;s capital city is Onverwacht, with other towns including Paranam, Sabana and Zanderij.</obo:IAO_0000115>
        <rdfs:label>Para District</rdfs:label>
        <oboInOwl:hasOBONamespace>GAZ</oboInOwl:hasOBONamespace>
        <oboInOwl:id>GAZ:00000089</oboInOwl:id>
    </rdf:Description>
    <rdf:Description rdf:about="http://purl.obolibrary.org/obo/GAZ_00000090">
        <oboInOwl:hasOBONamespace>GAZ</oboInOwl:hasOBONamespace>
        <rdfs:label>Saramacca District</rdfs:label>
        <oboInOwl:id>GAZ:00000090</oboInOwl:id>
        <obo:IAO_0000115>A district of Suriname, in the north. Saramacca&apos;s capital city is Groningen, with other towns and cities including Batavia and Boskamp.</obo:IAO_0000115>
    </rdf:Description>
    <rdf:Description rdf:about="http://purl.obolibrary.org/obo/GAZ_00000091">
        <oboInOwl:id>GAZ:00000091</oboInOwl:id>
        <oboInOwl:hasOBONamespace>GAZ</oboInOwl:hasOBONamespace>
        <obo:IAO_0000115>The largest district of Suriname, located in the south. Sipaliwini does not have a regional capital as it is directly administered by the national government in Paramaribo. The main villages in the district are Apetina, Apoera, Bakhuys, Bitagron, Pokigron, Kajana, Kamp 52, Pelelu Tepu, Cottica, Anapaike, Benzdorp, Kwamalasamutu, Nieuw Jacobkondre, Aurora, Botopasi, Goddo, Djumu and Pontoetoe.</obo:IAO_0000115>
        <rdfs:label>Sipaliwini District</rdfs:label>
    </rdf:Description>
    <rdf:Description rdf:about="http://purl.obolibrary.org/obo/GAZ_00000093">
        <oboInOwl:id>GAZ:00000093</oboInOwl:id>
        <oboInOwl:hasOBONamespace>GAZ</oboInOwl:hasOBONamespace>
        <rdfs:label>Matta</rdfs:label>
    </rdf:Description>
    <rdf:Description rdf:about="http://purl.obolibrary.org/obo/GAZ_00005322">
        <oboInOwl:id>GAZ:00005322</oboInOwl:id>
        <rdfs:label>populated place, Surinam</rdfs:label>
        <oboInOwl:hasOBONamespace>GAZ</oboInOwl:hasOBONamespace>
    </rdf:Description>
    <rdf:Description rdf:about="http://purl.obolibrary.org/obo/GAZ_00005323">
        <oboInOwl:id>GAZ:00005323</oboInOwl:id>
        <rdfs:label>District (Suriname)</rdfs:label>
        <oboInOwl:hasOBONamespace>GAZ</oboInOwl:hasOBONamespace>
    </rdf:Description>
    <rdf:Description rdf:about="http://purl.obolibrary.org/obo/GAZ_00005324">
        <rdfs:label>Paramaribo District</rdfs:label>
        <oboInOwl:id>GAZ:00005324</oboInOwl:id>
        <obo:IAO_0000115>A district of Suriname, encompassing the city of Paramaribo and the surrounding area. Het ligt ingeklemd tussen de districten Wanica in het westen en Commewijne in het oosten, en de monding van de rivier de Suriname in het noorden.</obo:IAO_0000115>
        <oboInOwl:hasOBONamespace>GAZ</oboInOwl:hasOBONamespace>
    </rdf:Description>
    <rdf:Description rdf:about="http://purl.obolibrary.org/obo/GAZ_00256506">
        <rdfs:label>Paramaribo</rdfs:label>
        <oboInOwl:id>GAZ:00256506</oboInOwl:id>
        <oboInOwl:hasOBONamespace>GAZ</oboInOwl:hasOBONamespace>
        <obo:IAO_0000115>A populated place. The capital and largest city of Suriname, located on banks of the Suriname River in the Paramaribo District.</obo:IAO_0000115>
    </rdf:Description>
</rdf:RDF>



<!-- Generated by the OWL API (version 4.5.6) https://github.com/owlcs/owlapi -->

