<?xml version="1.0"?>
<rdf:RDF xmlns="http://purl.obolibrary.org/obo/gaz/subsets/countries/Uganda.owl#"
     xml:base="http://purl.obolibrary.org/obo/gaz/subsets/countries/Uganda.owl"
     xmlns:obo="http://purl.obolibrary.org/obo/"
     xmlns:owl="http://www.w3.org/2002/07/owl#"
     xmlns:rdf="http://www.w3.org/1999/02/22-rdf-syntax-ns#"
     xmlns:xml="http://www.w3.org/XML/1998/namespace"
     xmlns:xsd="http://www.w3.org/2001/XMLSchema#"
     xmlns:rdfs="http://www.w3.org/2000/01/rdf-schema#"
     xmlns:oboInOwl="http://www.geneontology.org/formats/oboInOwl#">
    <owl:Ontology rdf:about="http://purl.obolibrary.org/obo/gaz/subsets/countries/Uganda.owl">
        <owl:imports rdf:resource="http://purl.obolibrary.org/obo/gaz/imports/envo_import.owl"/>
        <owl:imports rdf:resource="http://purl.obolibrary.org/obo/gaz/imports/ro_import.owl"/>
    </owl:Ontology>
    


    <!-- 
    ///////////////////////////////////////////////////////////////////////////////////////
    //
    // Annotation properties
    //
    ///////////////////////////////////////////////////////////////////////////////////////
     -->

    


    <!-- http://purl.obolibrary.org/obo/IAO_0000115 -->

    <owl:AnnotationProperty rdf:about="http://purl.obolibrary.org/obo/IAO_0000115"/>
    


    <!-- http://www.geneontology.org/formats/oboInOwl#hasOBONamespace -->

    <owl:AnnotationProperty rdf:about="http://www.geneontology.org/formats/oboInOwl#hasOBONamespace"/>
    


    <!-- http://www.geneontology.org/formats/oboInOwl#id -->

    <owl:AnnotationProperty rdf:about="http://www.geneontology.org/formats/oboInOwl#id"/>
    


    <!-- 
    ///////////////////////////////////////////////////////////////////////////////////////
    //
    // Object Properties
    //
    ///////////////////////////////////////////////////////////////////////////////////////
     -->

    


    <!-- http://purl.obolibrary.org/obo/RO_0001025 -->

    <owl:ObjectProperty rdf:about="http://purl.obolibrary.org/obo/RO_0001025"/>
    


    <!-- 
    ///////////////////////////////////////////////////////////////////////////////////////
    //
    // Classes
    //
    ///////////////////////////////////////////////////////////////////////////////////////
     -->

    


    <!-- http://purl.obolibrary.org/obo/ENVO_00000004 -->

    <owl:Class rdf:about="http://purl.obolibrary.org/obo/ENVO_00000004"/>
    


    <!-- http://purl.obolibrary.org/obo/ENVO_00000019 -->

    <owl:Class rdf:about="http://purl.obolibrary.org/obo/ENVO_00000019"/>
    


    <!-- http://purl.obolibrary.org/obo/ENVO_00000032 -->

    <owl:Class rdf:about="http://purl.obolibrary.org/obo/ENVO_00000032"/>
    


    <!-- http://purl.obolibrary.org/obo/ENVO_00000100 -->

    <owl:Class rdf:about="http://purl.obolibrary.org/obo/ENVO_00000100"/>
    


    <!-- http://purl.obolibrary.org/obo/ENVO_00000309 -->

    <owl:Class rdf:about="http://purl.obolibrary.org/obo/ENVO_00000309"/>
    


    <!-- http://purl.obolibrary.org/obo/ENVO_00000475 -->

    <owl:Class rdf:about="http://purl.obolibrary.org/obo/ENVO_00000475"/>
    


    <!-- http://purl.obolibrary.org/obo/ENVO_00000479 -->

    <owl:Class rdf:about="http://purl.obolibrary.org/obo/ENVO_00000479"/>
    


    <!-- http://purl.obolibrary.org/obo/ENVO_00000856 -->

    <owl:Class rdf:about="http://purl.obolibrary.org/obo/ENVO_00000856"/>
    


    <!-- http://purl.obolibrary.org/obo/GAZ_00005373 -->

    <owl:Class rdf:about="http://purl.obolibrary.org/obo/GAZ_00005373"/>
    


    <!-- http://purl.obolibrary.org/obo/GAZ_00005374 -->

    <owl:Class rdf:about="http://purl.obolibrary.org/obo/GAZ_00005374">
        <rdfs:subClassOf rdf:resource="http://purl.obolibrary.org/obo/GAZ_00005373"/>
    </owl:Class>
    


    <!-- http://purl.obolibrary.org/obo/GAZ_00005375 -->

    <owl:Class rdf:about="http://purl.obolibrary.org/obo/GAZ_00005375">
        <rdfs:subClassOf rdf:resource="http://purl.obolibrary.org/obo/GAZ_00005373"/>
    </owl:Class>
    


    <!-- http://purl.obolibrary.org/obo/GAZ_00005376 -->

    <owl:Class rdf:about="http://purl.obolibrary.org/obo/GAZ_00005376">
        <rdfs:subClassOf rdf:resource="http://purl.obolibrary.org/obo/GAZ_00005373"/>
    </owl:Class>
    


    <!-- http://purl.obolibrary.org/obo/GAZ_00005377 -->

    <owl:Class rdf:about="http://purl.obolibrary.org/obo/GAZ_00005377">
        <rdfs:subClassOf rdf:resource="http://purl.obolibrary.org/obo/GAZ_00005373"/>
    </owl:Class>
    


    <!-- http://purl.obolibrary.org/obo/GAZ_00005381 -->

    <owl:Class rdf:about="http://purl.obolibrary.org/obo/GAZ_00005381">
        <rdfs:subClassOf rdf:resource="http://purl.obolibrary.org/obo/GAZ_00005382"/>
    </owl:Class>
    


    <!-- http://purl.obolibrary.org/obo/GAZ_00005382 -->

    <owl:Class rdf:about="http://purl.obolibrary.org/obo/GAZ_00005382"/>
    


    <!-- http://purl.obolibrary.org/obo/GAZ_00009914 -->

    <owl:Class rdf:about="http://purl.obolibrary.org/obo/GAZ_00009914">
        <rdfs:subClassOf rdf:resource="http://purl.obolibrary.org/obo/GAZ_00005382"/>
    </owl:Class>
    


    <!-- http://purl.obolibrary.org/obo/GAZ_00009916 -->

    <owl:Class rdf:about="http://purl.obolibrary.org/obo/GAZ_00009916">
        <rdfs:subClassOf rdf:resource="http://purl.obolibrary.org/obo/GAZ_00005382"/>
    </owl:Class>
    


    <!-- http://purl.obolibrary.org/obo/GAZ_00009918 -->

    <owl:Class rdf:about="http://purl.obolibrary.org/obo/GAZ_00009918">
        <rdfs:subClassOf rdf:resource="http://purl.obolibrary.org/obo/GAZ_00005382"/>
    </owl:Class>
    


    <!-- http://purl.obolibrary.org/obo/GAZ_00015413 -->

    <owl:Class rdf:about="http://purl.obolibrary.org/obo/GAZ_00015413"/>
    


    <!-- http://purl.obolibrary.org/obo/GAZ_00236580 -->

    <owl:Class rdf:about="http://purl.obolibrary.org/obo/GAZ_00236580">
        <rdfs:subClassOf rdf:resource="http://purl.obolibrary.org/obo/GAZ_00015413"/>
        <obo:IAO_0000115>A fourth-level administrative division of Uganda.</obo:IAO_0000115>
        <oboInOwl:hasOBONamespace>GAZ</oboInOwl:hasOBONamespace>
        <oboInOwl:id>GAZ:00236580</oboInOwl:id>
        <rdfs:label>Entebbe Division A</rdfs:label>
    </owl:Class>
    


    <!-- http://purl.obolibrary.org/obo/GAZ_00236581 -->

    <owl:Class rdf:about="http://purl.obolibrary.org/obo/GAZ_00236581">
        <rdfs:subClassOf rdf:resource="http://purl.obolibrary.org/obo/GAZ_00015413"/>
        <obo:IAO_0000115>A fourth-level administrative division of Uganda.</obo:IAO_0000115>
        <oboInOwl:hasOBONamespace>GAZ</oboInOwl:hasOBONamespace>
        <oboInOwl:id>GAZ:00236581</oboInOwl:id>
        <rdfs:label>Entebbe Division B</rdfs:label>
    </owl:Class>
    


    <!-- 
    ///////////////////////////////////////////////////////////////////////////////////////
    //
    // Individuals
    //
    ///////////////////////////////////////////////////////////////////////////////////////
     -->

    


    <!-- http://purl.obolibrary.org/obo/GAZ_00000007 -->

    <owl:NamedIndividual rdf:about="http://purl.obolibrary.org/obo/GAZ_00000007">
        <obo:IAO_0000115>A rift valley. A geographical and geological feature, approximately 6,000 km in length, that runs from northern Syria in Southwest Asia to central Mozambique in East Africa.</obo:IAO_0000115>
        <oboInOwl:hasOBONamespace>GAZ</oboInOwl:hasOBONamespace>
        <oboInOwl:id>GAZ:00000007</oboInOwl:id>
        <rdfs:label>Great Rift Valley</rdfs:label>
    </owl:NamedIndividual>
    


    <!-- http://purl.obolibrary.org/obo/GAZ_00000008 -->

    <owl:NamedIndividual rdf:about="http://purl.obolibrary.org/obo/GAZ_00000008">
        <obo:RO_0001025 rdf:resource="http://purl.obolibrary.org/obo/GAZ_00000007"/>
        <obo:IAO_0000115>A soda lake, in the eastern part of the Great Rift Valley. A Ramsar Site.</obo:IAO_0000115>
        <oboInOwl:hasOBONamespace>GAZ</oboInOwl:hasOBONamespace>
        <oboInOwl:id>GAZ:00000008</oboInOwl:id>
        <rdfs:label>Lake Elmenteita</rdfs:label>
    </owl:NamedIndividual>
    


    <!-- http://purl.obolibrary.org/obo/GAZ_00000058 -->

    <owl:NamedIndividual rdf:about="http://purl.obolibrary.org/obo/GAZ_00000058">
        <obo:RO_0001025 rdf:resource="http://purl.obolibrary.org/obo/GAZ_00000007"/>
        <obo:IAO_0000115>A freshwater lake that is the most southerly lake in the Great African Rift Valley system. Its largest tributary is the Ruhuhu and its outlet is the Shire River, a tributary of the Zambezi.</obo:IAO_0000115>
        <oboInOwl:hasOBONamespace>GAZ</oboInOwl:hasOBONamespace>
        <oboInOwl:id>GAZ:00000058</oboInOwl:id>
        <rdfs:label>Lake Malawi</rdfs:label>
    </owl:NamedIndividual>
    


    <!-- http://purl.obolibrary.org/obo/GAZ_00001102 -->

    <owl:NamedIndividual rdf:about="http://purl.obolibrary.org/obo/GAZ_00001102">
        <obo:IAO_0000115>A landlocked country in East Africa, bordered on the east by Kenya, the north by Sudan, on the west by the Democratic Republic of the Congo, on the southwest by Rwanda, and on the south by Tanzania. The southern part of the country includes a substantial portion of Lake Victoria, within which it shares borders with Kenya and Tanzania. Uganda is divided into 80 districts, spread across four administrative regions: Northern, Eastern, Central and Western. The districts are subdivided into counties.</obo:IAO_0000115>
        <oboInOwl:hasOBONamespace>GAZ</oboInOwl:hasOBONamespace>
        <oboInOwl:id>GAZ:00001102</oboInOwl:id>
        <rdfs:label>Uganda</rdfs:label>
    </owl:NamedIndividual>
    


    <!-- http://purl.obolibrary.org/obo/GAZ_00002477 -->

    <owl:NamedIndividual rdf:about="http://purl.obolibrary.org/obo/GAZ_00002477">
        <obo:RO_0001025 rdf:resource="http://purl.obolibrary.org/obo/GAZ_00007520"/>
        <obo:IAO_0000115>A saline lake between the West Bank and Israel to the west, and Jordan to the east.</obo:IAO_0000115>
        <oboInOwl:hasOBONamespace>GAZ</oboInOwl:hasOBONamespace>
        <oboInOwl:id>GAZ:00002477</oboInOwl:id>
        <rdfs:label>Dead Sea</rdfs:label>
    </owl:NamedIndividual>
    


    <!-- http://purl.obolibrary.org/obo/GAZ_00005373 -->

    <owl:NamedIndividual rdf:about="http://purl.obolibrary.org/obo/GAZ_00005373">
        <obo:RO_0001025 rdf:resource="http://purl.obolibrary.org/obo/GAZ_00001102"/>
    </owl:NamedIndividual>
    


    <!-- http://purl.obolibrary.org/obo/GAZ_00005374 -->

    <owl:NamedIndividual rdf:about="http://purl.obolibrary.org/obo/GAZ_00005374"/>
    


    <!-- http://purl.obolibrary.org/obo/GAZ_00005375 -->

    <owl:NamedIndividual rdf:about="http://purl.obolibrary.org/obo/GAZ_00005375"/>
    


    <!-- http://purl.obolibrary.org/obo/GAZ_00005376 -->

    <owl:NamedIndividual rdf:about="http://purl.obolibrary.org/obo/GAZ_00005376"/>
    


    <!-- http://purl.obolibrary.org/obo/GAZ_00005377 -->

    <owl:NamedIndividual rdf:about="http://purl.obolibrary.org/obo/GAZ_00005377"/>
    


    <!-- http://purl.obolibrary.org/obo/GAZ_00005378 -->

    <owl:NamedIndividual rdf:about="http://purl.obolibrary.org/obo/GAZ_00005378">
        <rdf:type rdf:resource="http://purl.obolibrary.org/obo/ENVO_00000004"/>
        <obo:RO_0001025 rdf:resource="http://purl.obolibrary.org/obo/GAZ_00005377"/>
        <obo:IAO_0000115>A district in central Uganda. Mpigi District is bordered by Wakiso District to the east, Kalangala District and Masaka District to the south, Sembabule District to the southwest, Mubende District to the northwest and Mityana District to the north.</obo:IAO_0000115>
        <oboInOwl:hasOBONamespace>GAZ</oboInOwl:hasOBONamespace>
        <oboInOwl:id>GAZ:00005378</oboInOwl:id>
        <rdfs:label>Mpigi District</rdfs:label>
    </owl:NamedIndividual>
    


    <!-- http://purl.obolibrary.org/obo/GAZ_00005379 -->

    <owl:NamedIndividual rdf:about="http://purl.obolibrary.org/obo/GAZ_00005379">
        <obo:RO_0001025 rdf:resource="http://purl.obolibrary.org/obo/GAZ_00005378"/>
        <obo:IAO_0000115>A protected area located 37 km west from Kampala along the Masaka Road.</obo:IAO_0000115>
        <oboInOwl:hasOBONamespace>GAZ</oboInOwl:hasOBONamespace>
        <oboInOwl:id>GAZ:00005379</oboInOwl:id>
        <rdfs:label>Mpanga Forest Reserve</rdfs:label>
    </owl:NamedIndividual>
    


    <!-- http://purl.obolibrary.org/obo/GAZ_00005380 -->

    <owl:NamedIndividual rdf:about="http://purl.obolibrary.org/obo/GAZ_00005380">
        <rdf:type rdf:resource="http://purl.obolibrary.org/obo/ENVO_00000004"/>
        <obo:RO_0001025 rdf:resource="http://purl.obolibrary.org/obo/GAZ_00005377"/>
        <obo:IAO_0000115>A district in central Uganda. The district is bordered by Sembabule District in the northwest, Mpigi District in the north, Rakai District in the west and south and Kalangala District in the east.</obo:IAO_0000115>
        <oboInOwl:hasOBONamespace>GAZ</oboInOwl:hasOBONamespace>
        <oboInOwl:id>GAZ:00005380</oboInOwl:id>
        <rdfs:label>Masaka District</rdfs:label>
    </owl:NamedIndividual>
    


    <!-- http://purl.obolibrary.org/obo/GAZ_00005381 -->

    <owl:NamedIndividual rdf:about="http://purl.obolibrary.org/obo/GAZ_00005381">
        <obo:RO_0001025 rdf:resource="http://purl.obolibrary.org/obo/GAZ_00012976"/>
    </owl:NamedIndividual>
    


    <!-- http://purl.obolibrary.org/obo/GAZ_00005382 -->

    <owl:NamedIndividual rdf:about="http://purl.obolibrary.org/obo/GAZ_00005382">
        <obo:RO_0001025 rdf:resource="http://purl.obolibrary.org/obo/GAZ_00001102"/>
    </owl:NamedIndividual>
    


    <!-- http://purl.obolibrary.org/obo/GAZ_00007520 -->

    <owl:NamedIndividual rdf:about="http://purl.obolibrary.org/obo/GAZ_00007520">
        <obo:RO_0001025 rdf:resource="http://purl.obolibrary.org/obo/GAZ_00044915"/>
        <obo:IAO_0000115>A river in Southwest Asia flowing through the Great Rift Valley into the Dead Sea.</obo:IAO_0000115>
        <oboInOwl:hasOBONamespace>GAZ</oboInOwl:hasOBONamespace>
        <oboInOwl:id>GAZ:00007520</oboInOwl:id>
        <rdfs:label>River Jordan</rdfs:label>
    </owl:NamedIndividual>
    


    <!-- http://purl.obolibrary.org/obo/GAZ_00007523 -->

    <owl:NamedIndividual rdf:about="http://purl.obolibrary.org/obo/GAZ_00007523">
        <obo:RO_0001025 rdf:resource="http://purl.obolibrary.org/obo/GAZ_00000007"/>
        <obo:IAO_0000115>A saline, alkaline lake, approximately 100 km2 in size, that lies in a graben. The lake is an example of a &quot;saline pan&quot;. The lake water, which is a dense sodium carbonate brine, precipitates vast quanitites of the mineral called trona (sodium sesquicarbonate). In places, the salt is up to 40 m thick. The lake is recharged mainly by saline hot springs (temperatures up to about 83degC) that discharge into alkaline &quot;lagoons&quot; around the lake margins, there being little surface runoff in this arid region. Most hot springs lie along the northwestern and southern shorelines of the lake. During the rainy season a thin (&lt;1m) layer of brine covers much of the saline pan, but this evaporates rapidly leaving a vast expanse of white salt that cracks to produce large polygons.</obo:IAO_0000115>
        <oboInOwl:hasOBONamespace>GAZ</oboInOwl:hasOBONamespace>
        <oboInOwl:id>GAZ:00007523</oboInOwl:id>
        <rdfs:label>Lake Magadi</rdfs:label>
    </owl:NamedIndividual>
    


    <!-- http://purl.obolibrary.org/obo/GAZ_00007862 -->

    <owl:NamedIndividual rdf:about="http://purl.obolibrary.org/obo/GAZ_00007862">
        <rdf:type rdf:resource="http://purl.obolibrary.org/obo/ENVO_00000032"/>
        <obo:RO_0001025 rdf:resource="http://purl.obolibrary.org/obo/GAZ_00000007"/>
        <obo:IAO_0000115>A gulf situated northeastward and adjacent to the Red Sea, bounded by the coasts of Sinai Peninsula and Arabian Peninsula. Its southern limit with the Red Sea (in the Strait of T Degrees r Degrees n) is the following: A line joining Cape Al Qa Degrees bah (28 Degrees 01430 Seconds N - 34 Degrees 37 Minutes 15 Seconds E), in Saudi Arabia, southwestward to position 27 Degrees 58 Minutes 10 Seconds N - 34 Degrees 35 Minutes E) on the coast of T Degrees r Degrees n Island; thence from this position southward, through T Degrees r Degrees n Island, to its southwestern extremity (27 Degrees 54 Minutes 50 Seconds N - 34 Degrees 33 Minutes E); and thence from the southwestern extremity of T Degrees r Degrees n Island westward, along the parallel of 27 Degrees 54 Minutes 50 Seconds N, to the coast of Sinai Peninsula, in Egypt.</obo:IAO_0000115>
        <oboInOwl:hasOBONamespace>GAZ</oboInOwl:hasOBONamespace>
        <oboInOwl:id>GAZ:00007862</oboInOwl:id>
        <rdfs:label>Gulf of Aqaba</rdfs:label>
    </owl:NamedIndividual>
    


    <!-- http://purl.obolibrary.org/obo/GAZ_00008411 -->

    <owl:NamedIndividual rdf:about="http://purl.obolibrary.org/obo/GAZ_00008411">
        <obo:RO_0001025 rdf:resource="http://purl.obolibrary.org/obo/GAZ_00000007"/>
        <obo:IAO_0000115>A saline, alkaline lake that lies in a volcanic region in a half-graben basin south of Lake Baringo, Kenya, a little north of the equator. A Ramsar Site.</obo:IAO_0000115>
        <oboInOwl:hasOBONamespace>GAZ</oboInOwl:hasOBONamespace>
        <oboInOwl:id>GAZ:00008411</oboInOwl:id>
        <rdfs:label>Lake Bogoria</rdfs:label>
    </owl:NamedIndividual>
    


    <!-- http://purl.obolibrary.org/obo/GAZ_00008558 -->

    <owl:NamedIndividual rdf:about="http://purl.obolibrary.org/obo/GAZ_00008558">
        <obo:RO_0001025 rdf:resource="http://purl.obolibrary.org/obo/GAZ_00000007"/>
        <obo:IAO_0000115>A meromictic lake that on the border between the Democratic Republic of the Congo and Rwanda, and is in the Albertine (western) Rift, a part of the Great Rift Valley. Lake Kivu empties into the Ruzizi River, which flows southwards into Lake Tanganyika.</obo:IAO_0000115>
        <oboInOwl:hasOBONamespace>GAZ</oboInOwl:hasOBONamespace>
        <oboInOwl:id>GAZ:00008558</oboInOwl:id>
        <rdfs:label>Lake Kivu</rdfs:label>
    </owl:NamedIndividual>
    


    <!-- http://purl.obolibrary.org/obo/GAZ_00008742 -->

    <owl:NamedIndividual rdf:about="http://purl.obolibrary.org/obo/GAZ_00008742">
        <obo:RO_0001025 rdf:resource="http://purl.obolibrary.org/obo/GAZ_00044915"/>
        <obo:IAO_0000115>A valley that lies within the northern part of the Syrian-African Rift Valley at an elevation of about 70 m above sea level. On both sides of the valley are steep slopes -- the Golan Heights to the east and the Upper Galilee mountains to the west, rise to 400 to 900 m above sea level. Basaltic hills of about 200 m above sea level along the southern side of the valley intercept the Jordan River, and are commonly referred to as the basalt &quot;plug&quot; (actually a temporary geologic base level), as they restrict water drainage downstream into the Sea of Galilee (Lake Kinneret). The Hula Valley covers an area of 177 km2 (25 km by 6-8 km.</obo:IAO_0000115>
        <oboInOwl:hasOBONamespace>GAZ</oboInOwl:hasOBONamespace>
        <oboInOwl:id>GAZ:00008742</oboInOwl:id>
        <rdfs:label>Hulah Valley</rdfs:label>
    </owl:NamedIndividual>
    


    <!-- http://purl.obolibrary.org/obo/GAZ_00008743 -->

    <owl:NamedIndividual rdf:about="http://purl.obolibrary.org/obo/GAZ_00008743">
        <obo:RO_0001025 rdf:resource="http://purl.obolibrary.org/obo/GAZ_00193886"/>
        <obo:IAO_0000115>A wetland.</obo:IAO_0000115>
        <oboInOwl:hasOBONamespace>GAZ</oboInOwl:hasOBONamespace>
        <oboInOwl:id>GAZ:00008743</oboInOwl:id>
        <rdfs:label>Hulah Swamp</rdfs:label>
    </owl:NamedIndividual>
    


    <!-- http://purl.obolibrary.org/obo/GAZ_00009142 -->

    <owl:NamedIndividual rdf:about="http://purl.obolibrary.org/obo/GAZ_00009142">
        <obo:RO_0001025 rdf:resource="http://purl.obolibrary.org/obo/GAZ_00008558"/>
        <obo:IAO_0000115>An island in Lake Kivu, belonging to the Democratic Republic of the Congo. At 40 km in length and with an area of 285 km2.</obo:IAO_0000115>
        <oboInOwl:hasOBONamespace>GAZ</oboInOwl:hasOBONamespace>
        <oboInOwl:id>GAZ:00009142</oboInOwl:id>
        <rdfs:label>Idjwi Island</rdfs:label>
    </owl:NamedIndividual>
    


    <!-- http://purl.obolibrary.org/obo/GAZ_00009913 -->

    <owl:NamedIndividual rdf:about="http://purl.obolibrary.org/obo/GAZ_00009913">
        <rdf:type rdf:resource="http://purl.obolibrary.org/obo/ENVO_00000004"/>
        <obo:RO_0001025 rdf:resource="http://purl.obolibrary.org/obo/GAZ_00236917"/>
        <obo:IAO_0000115>A district in northern Uganda.</obo:IAO_0000115>
        <oboInOwl:hasOBONamespace>GAZ</oboInOwl:hasOBONamespace>
        <oboInOwl:id>GAZ:00009913</oboInOwl:id>
        <rdfs:label>Gulu District</rdfs:label>
    </owl:NamedIndividual>
    


    <!-- http://purl.obolibrary.org/obo/GAZ_00009914 -->

    <owl:NamedIndividual rdf:about="http://purl.obolibrary.org/obo/GAZ_00009914">
        <obo:RO_0001025 rdf:resource="http://purl.obolibrary.org/obo/GAZ_00012974"/>
    </owl:NamedIndividual>
    


    <!-- http://purl.obolibrary.org/obo/GAZ_00009915 -->

    <owl:NamedIndividual rdf:about="http://purl.obolibrary.org/obo/GAZ_00009915">
        <rdf:type rdf:resource="http://purl.obolibrary.org/obo/ENVO_00000004"/>
        <obo:RO_0001025 rdf:resource="http://purl.obolibrary.org/obo/GAZ_00005374"/>
        <obo:IAO_0000115>A district in western Uganda. Masindi District is bordered by Amuru District to the north, Oyam District to the northeast, Apac District to the east, Nakasongola District and Nakaseke District to the southeast, Kiboga District to the south, Hoima District to the southwest and Bulisa District to the northwest.</obo:IAO_0000115>
        <oboInOwl:hasOBONamespace>GAZ</oboInOwl:hasOBONamespace>
        <oboInOwl:id>GAZ:00009915</oboInOwl:id>
        <rdfs:label>Masindi District</rdfs:label>
    </owl:NamedIndividual>
    


    <!-- http://purl.obolibrary.org/obo/GAZ_00009916 -->

    <owl:NamedIndividual rdf:about="http://purl.obolibrary.org/obo/GAZ_00009916">
        <obo:RO_0001025 rdf:resource="http://purl.obolibrary.org/obo/GAZ_00237349"/>
    </owl:NamedIndividual>
    


    <!-- http://purl.obolibrary.org/obo/GAZ_00009917 -->

    <owl:NamedIndividual rdf:about="http://purl.obolibrary.org/obo/GAZ_00009917">
        <rdf:type rdf:resource="http://purl.obolibrary.org/obo/ENVO_00000004"/>
        <obo:RO_0001025 rdf:resource="http://purl.obolibrary.org/obo/GAZ_00005374"/>
        <obo:IAO_0000115>A district in southwestern Uganda. Mbarara district is bordered by the districts of Ntungamo, Sembabule, Rakai, Bushenyi.</obo:IAO_0000115>
        <oboInOwl:hasOBONamespace>GAZ</oboInOwl:hasOBONamespace>
        <oboInOwl:id>GAZ:00009917</oboInOwl:id>
        <rdfs:label>Mbarara District</rdfs:label>
    </owl:NamedIndividual>
    


    <!-- http://purl.obolibrary.org/obo/GAZ_00009918 -->

    <owl:NamedIndividual rdf:about="http://purl.obolibrary.org/obo/GAZ_00009918">
        <obo:RO_0001025 rdf:resource="http://purl.obolibrary.org/obo/GAZ_00012975"/>
    </owl:NamedIndividual>
    


    <!-- http://purl.obolibrary.org/obo/GAZ_00010533 -->

    <owl:NamedIndividual rdf:about="http://purl.obolibrary.org/obo/GAZ_00010533">
        <obo:RO_0001025 rdf:resource="http://purl.obolibrary.org/obo/GAZ_00044915"/>
        <obo:IAO_0000115>A large fertile plain and inland valley in the south of the Lower Galilee region of Israel. It is bordered to the south by the Samaria highlands and Mount Gilboa, to the north by the Lower Galilee, to the west by the Mount Carmel range, and to the east by the Jordan Valley.</obo:IAO_0000115>
        <oboInOwl:hasOBONamespace>GAZ</oboInOwl:hasOBONamespace>
        <oboInOwl:id>GAZ:00010533</oboInOwl:id>
        <rdfs:label>Jezreel Valley</rdfs:label>
    </owl:NamedIndividual>
    


    <!-- http://purl.obolibrary.org/obo/GAZ_00011722 -->

    <owl:NamedIndividual rdf:about="http://purl.obolibrary.org/obo/GAZ_00011722">
        <obo:RO_0001025 rdf:resource="http://purl.obolibrary.org/obo/GAZ_00000007"/>
        <obo:IAO_0000115>A freshwater lake is situated within the Western Rift of the Great Rift Valley. The major inflows are the Ruzizi River, entering the north of the lake from Lake Kivu, and the Malagarasi River, which is Tanzania&apos;s second largest river, entering in the east side of Lake Tanganyika. The Malagarasi pre-dates Lake Tanganyika and was formerly continuous with the Congo river.</obo:IAO_0000115>
        <oboInOwl:hasOBONamespace>GAZ</oboInOwl:hasOBONamespace>
        <oboInOwl:id>GAZ:00011722</oboInOwl:id>
        <rdfs:label>Lake Tanganyika</rdfs:label>
    </owl:NamedIndividual>
    


    <!-- http://purl.obolibrary.org/obo/GAZ_00012974 -->

    <owl:NamedIndividual rdf:about="http://purl.obolibrary.org/obo/GAZ_00012974">
        <obo:RO_0001025 rdf:resource="http://purl.obolibrary.org/obo/GAZ_00009913"/>
        <oboInOwl:hasOBONamespace>GAZ</oboInOwl:hasOBONamespace>
        <oboInOwl:id>GAZ:00012974</oboInOwl:id>
        <rdfs:label>Gulu County</rdfs:label>
    </owl:NamedIndividual>
    


    <!-- http://purl.obolibrary.org/obo/GAZ_00012975 -->

    <owl:NamedIndividual rdf:about="http://purl.obolibrary.org/obo/GAZ_00012975">
        <obo:RO_0001025 rdf:resource="http://purl.obolibrary.org/obo/GAZ_00009917"/>
        <oboInOwl:hasOBONamespace>GAZ</oboInOwl:hasOBONamespace>
        <oboInOwl:id>GAZ:00012975</oboInOwl:id>
        <rdfs:label>Municipality of Mbarara</rdfs:label>
    </owl:NamedIndividual>
    


    <!-- http://purl.obolibrary.org/obo/GAZ_00012976 -->

    <owl:NamedIndividual rdf:about="http://purl.obolibrary.org/obo/GAZ_00012976">
        <obo:RO_0001025 rdf:resource="http://purl.obolibrary.org/obo/GAZ_00005380"/>
        <oboInOwl:hasOBONamespace>GAZ</oboInOwl:hasOBONamespace>
        <oboInOwl:id>GAZ:00012976</oboInOwl:id>
        <rdfs:label>Masaka Municipality</rdfs:label>
    </owl:NamedIndividual>
    


    <!-- http://purl.obolibrary.org/obo/GAZ_00015337 -->

    <owl:NamedIndividual rdf:about="http://purl.obolibrary.org/obo/GAZ_00015337">
        <obo:RO_0001025 rdf:resource="http://purl.obolibrary.org/obo/GAZ_00015427"/>
        <oboInOwl:hasOBONamespace>GAZ</oboInOwl:hasOBONamespace>
        <oboInOwl:id>GAZ:00015337</oboInOwl:id>
        <rdfs:label>Lyantonde Sub-county</rdfs:label>
    </owl:NamedIndividual>
    


    <!-- http://purl.obolibrary.org/obo/GAZ_00015338 -->

    <owl:NamedIndividual rdf:about="http://purl.obolibrary.org/obo/GAZ_00015338">
        <rdf:type rdf:resource="http://purl.obolibrary.org/obo/ENVO_00000004"/>
        <obo:RO_0001025 rdf:resource="http://purl.obolibrary.org/obo/GAZ_00005377"/>
        <obo:IAO_0000115>A district in Uganda that almost encircles Kampala, Uganda&apos;s capital city. Wakiso District lies in the central region of the country, bordering with Luwero District in the north, Nakaseke in the northeast, Mityana District in the west, Mpigi District in the west and southwest and Kalangala District in Lake Victoria to the south.</obo:IAO_0000115>
        <oboInOwl:hasOBONamespace>GAZ</oboInOwl:hasOBONamespace>
        <oboInOwl:id>GAZ:00015338</oboInOwl:id>
        <rdfs:label>Wakiso District</rdfs:label>
    </owl:NamedIndividual>
    


    <!-- http://purl.obolibrary.org/obo/GAZ_00015339 -->

    <owl:NamedIndividual rdf:about="http://purl.obolibrary.org/obo/GAZ_00015339">
        <rdf:type rdf:resource="http://purl.obolibrary.org/obo/ENVO_00000004"/>
        <obo:RO_0001025 rdf:resource="http://purl.obolibrary.org/obo/GAZ_00005377"/>
        <obo:IAO_0000115>A district in central Uganda. Mubende District is bordered by Mityana District to the east, Kiboga District to the north, Kibaale District to the northwest, Kyenjojo District to the west, Sembabule District and Mpigi District to the south.</obo:IAO_0000115>
        <oboInOwl:hasOBONamespace>GAZ</oboInOwl:hasOBONamespace>
        <oboInOwl:id>GAZ:00015339</oboInOwl:id>
        <rdfs:label>Mubende District</rdfs:label>
    </owl:NamedIndividual>
    


    <!-- http://purl.obolibrary.org/obo/GAZ_00015340 -->

    <owl:NamedIndividual rdf:about="http://purl.obolibrary.org/obo/GAZ_00015340">
        <rdf:type rdf:resource="http://purl.obolibrary.org/obo/ENVO_00000004"/>
        <obo:RO_0001025 rdf:resource="http://purl.obolibrary.org/obo/GAZ_00005377"/>
        <obo:IAO_0000115>A district in central Uganda. Luwero District is bordered by Kayunga District to the northeast, Mukono District to the southeast, Wakiso District to the south, Nakaseke District to the west, and Nakasongola District to the north.</obo:IAO_0000115>
        <oboInOwl:hasOBONamespace>GAZ</oboInOwl:hasOBONamespace>
        <oboInOwl:id>GAZ:00015340</oboInOwl:id>
        <rdfs:label>Luwero Distroct</rdfs:label>
    </owl:NamedIndividual>
    


    <!-- http://purl.obolibrary.org/obo/GAZ_00015341 -->

    <owl:NamedIndividual rdf:about="http://purl.obolibrary.org/obo/GAZ_00015341">
        <rdf:type rdf:resource="http://purl.obolibrary.org/obo/ENVO_00000004"/>
        <obo:RO_0001025 rdf:resource="http://purl.obolibrary.org/obo/GAZ_00005377"/>
        <obo:IAO_0000115>A district in central Uganda. The district is bordered by Mukono District in the south, Jinja District in he east, Kamuli District in the northeast, Apac District in the north, Nakasongola District in the northwest and Luweero District in the west.</obo:IAO_0000115>
        <oboInOwl:hasOBONamespace>GAZ</oboInOwl:hasOBONamespace>
        <oboInOwl:id>GAZ:00015341</oboInOwl:id>
        <rdfs:label>Kayunga District</rdfs:label>
    </owl:NamedIndividual>
    


    <!-- http://purl.obolibrary.org/obo/GAZ_00015342 -->

    <owl:NamedIndividual rdf:about="http://purl.obolibrary.org/obo/GAZ_00015342">
        <rdf:type rdf:resource="http://purl.obolibrary.org/obo/ENVO_00000004"/>
        <obo:RO_0001025 rdf:resource="http://purl.obolibrary.org/obo/GAZ_00005377"/>
        <obo:IAO_0000115>A district in central Uganda. Mukono District is bordered by Jinja District and Jinja Municipality and Mayuge District to the east, the Republic of Tanzania to the south, Kalangala District to the southwest, Wakiso District and Kira Town to the west, Luweero District to the northwest and Kayunga District to the north. The Buvuma Islands in Lake Victoria are part of Mukono District.</obo:IAO_0000115>
        <oboInOwl:hasOBONamespace>GAZ</oboInOwl:hasOBONamespace>
        <oboInOwl:id>GAZ:00015342</oboInOwl:id>
        <rdfs:label>Mukono District</rdfs:label>
    </owl:NamedIndividual>
    


    <!-- http://purl.obolibrary.org/obo/GAZ_00015343 -->

    <owl:NamedIndividual rdf:about="http://purl.obolibrary.org/obo/GAZ_00015343">
        <rdf:type rdf:resource="http://purl.obolibrary.org/obo/ENVO_00000004"/>
        <obo:RO_0001025 rdf:resource="http://purl.obolibrary.org/obo/GAZ_00005377"/>
        <obo:IAO_0000115>A district in central Uganda. Kiboga District is bordered by Masindi District to the north, Nakaseke District to the east, Mityana District to the southeast, Mubende District to the south, Kibale District to the west and Hoima District to the northwest.</obo:IAO_0000115>
        <oboInOwl:hasOBONamespace>GAZ</oboInOwl:hasOBONamespace>
        <oboInOwl:id>GAZ:00015343</oboInOwl:id>
        <rdfs:label>Kiboga District</rdfs:label>
    </owl:NamedIndividual>
    


    <!-- http://purl.obolibrary.org/obo/GAZ_00015344 -->

    <owl:NamedIndividual rdf:about="http://purl.obolibrary.org/obo/GAZ_00015344">
        <rdf:type rdf:resource="http://purl.obolibrary.org/obo/ENVO_00000004"/>
        <obo:RO_0001025 rdf:resource="http://purl.obolibrary.org/obo/GAZ_00005377"/>
        <obo:IAO_0000115>A district in central Uganda. Kalangala District is bordered by Mpigi District and Wakiso District to the north, Mukono District to the northeast and east, the Republic of Tanzania to the south, Rakai District to the southwest and Masaka District to the west.</obo:IAO_0000115>
        <oboInOwl:hasOBONamespace>GAZ</oboInOwl:hasOBONamespace>
        <oboInOwl:id>GAZ:00015344</oboInOwl:id>
        <rdfs:label>Kalangala District</rdfs:label>
    </owl:NamedIndividual>
    


    <!-- http://purl.obolibrary.org/obo/GAZ_00015345 -->

    <owl:NamedIndividual rdf:about="http://purl.obolibrary.org/obo/GAZ_00015345">
        <rdf:type rdf:resource="http://purl.obolibrary.org/obo/ENVO_00000004"/>
        <obo:RO_0001025 rdf:resource="http://purl.obolibrary.org/obo/GAZ_00005377"/>
        <obo:IAO_0000115>A district in south-central Uganda. Rakai District borders Kagera Region in Tanzania to the south, Kalangala District, Masaka District and Sembabule District to the east, Sembabule District to the north, Kiruhura District to the northwest and Isingiro District the southwest.</obo:IAO_0000115>
        <oboInOwl:hasOBONamespace>GAZ</oboInOwl:hasOBONamespace>
        <oboInOwl:id>GAZ:00015345</oboInOwl:id>
        <rdfs:label>Rakai District</rdfs:label>
    </owl:NamedIndividual>
    


    <!-- http://purl.obolibrary.org/obo/GAZ_00015346 -->

    <owl:NamedIndividual rdf:about="http://purl.obolibrary.org/obo/GAZ_00015346">
        <rdf:type rdf:resource="http://purl.obolibrary.org/obo/ENVO_00000004"/>
        <obo:RO_0001025 rdf:resource="http://purl.obolibrary.org/obo/GAZ_00005377"/>
        <obo:IAO_0000115>A district in the Central Region of Uganda. Nakaseke District is bordered by Luweero District to the southeast and east, Nakasongola District to the northeast and north, Masindi District to the northwest, Kiboga District to the west and Mityana District to the south.</obo:IAO_0000115>
        <oboInOwl:hasOBONamespace>GAZ</oboInOwl:hasOBONamespace>
        <oboInOwl:id>GAZ:00015346</oboInOwl:id>
        <rdfs:label>Nakaseke District</rdfs:label>
    </owl:NamedIndividual>
    


    <!-- http://purl.obolibrary.org/obo/GAZ_00015347 -->

    <owl:NamedIndividual rdf:about="http://purl.obolibrary.org/obo/GAZ_00015347">
        <rdf:type rdf:resource="http://purl.obolibrary.org/obo/ENVO_00000004"/>
        <obo:RO_0001025 rdf:resource="http://purl.obolibrary.org/obo/GAZ_00005377"/>
        <obo:IAO_0000115>A district in the Central Region of Uganda. Mityana District is bordered by Wakiso District in the east, Nakaseke District in the northeast, Kiboga District in the north, Mubende District in the west and Mpigi District in the south and southeast.</obo:IAO_0000115>
        <oboInOwl:hasOBONamespace>GAZ</oboInOwl:hasOBONamespace>
        <oboInOwl:id>GAZ:00015347</oboInOwl:id>
        <rdfs:label>Mityana District</rdfs:label>
    </owl:NamedIndividual>
    


    <!-- http://purl.obolibrary.org/obo/GAZ_00015348 -->

    <owl:NamedIndividual rdf:about="http://purl.obolibrary.org/obo/GAZ_00015348">
        <rdf:type rdf:resource="http://purl.obolibrary.org/obo/ENVO_00000004"/>
        <obo:RO_0001025 rdf:resource="http://purl.obolibrary.org/obo/GAZ_00005377"/>
        <obo:IAO_0000115>A district in central Uganda. Nakasongola District is bordered by Apac District to the north, Masindi District to the west, Luwero District to the south and Kayunga District to the east.</obo:IAO_0000115>
        <oboInOwl:hasOBONamespace>GAZ</oboInOwl:hasOBONamespace>
        <oboInOwl:id>GAZ:00015348</oboInOwl:id>
        <rdfs:label>Nakasongola District</rdfs:label>
    </owl:NamedIndividual>
    


    <!-- http://purl.obolibrary.org/obo/GAZ_00015349 -->

    <owl:NamedIndividual rdf:about="http://purl.obolibrary.org/obo/GAZ_00015349">
        <rdf:type rdf:resource="http://purl.obolibrary.org/obo/ENVO_00000004"/>
        <obo:RO_0001025 rdf:resource="http://purl.obolibrary.org/obo/GAZ_00005377"/>
        <obo:IAO_0000115>A district in central Uganda. Sembabule District is bordered by Mubende District to the north, Mpigi District to the northeast, Masaka District to the east and south, Lyantonde District to the southwest and Kiruhura District to the west.</obo:IAO_0000115>
        <oboInOwl:hasOBONamespace>GAZ</oboInOwl:hasOBONamespace>
        <oboInOwl:id>GAZ:00015349</oboInOwl:id>
        <rdfs:label>Sembabule District</rdfs:label>
    </owl:NamedIndividual>
    


    <!-- http://purl.obolibrary.org/obo/GAZ_00015350 -->

    <owl:NamedIndividual rdf:about="http://purl.obolibrary.org/obo/GAZ_00015350">
        <rdf:type rdf:resource="http://purl.obolibrary.org/obo/ENVO_00000004"/>
        <obo:RO_0001025 rdf:resource="http://purl.obolibrary.org/obo/GAZ_00005377"/>
        <obo:IAO_0000115>A district in central Uganda.</obo:IAO_0000115>
        <oboInOwl:hasOBONamespace>GAZ</oboInOwl:hasOBONamespace>
        <oboInOwl:id>GAZ:00015350</oboInOwl:id>
        <rdfs:label>Kampala District</rdfs:label>
    </owl:NamedIndividual>
    


    <!-- http://purl.obolibrary.org/obo/GAZ_00015351 -->

    <owl:NamedIndividual rdf:about="http://purl.obolibrary.org/obo/GAZ_00015351">
        <rdf:type rdf:resource="http://purl.obolibrary.org/obo/ENVO_00000004"/>
        <obo:RO_0001025 rdf:resource="http://purl.obolibrary.org/obo/GAZ_00005376"/>
        <obo:IAO_0000115>A district in eastern Uganda. Jinja District is bordered Kamuli District to the north, Iganga District to the east, Mayuge District to the southeast, Mukono District to the west and Kayunga District to the northwest.</obo:IAO_0000115>
        <oboInOwl:hasOBONamespace>GAZ</oboInOwl:hasOBONamespace>
        <oboInOwl:id>GAZ:00015351</oboInOwl:id>
        <rdfs:label>Jinja District</rdfs:label>
    </owl:NamedIndividual>
    


    <!-- http://purl.obolibrary.org/obo/GAZ_00015352 -->

    <owl:NamedIndividual rdf:about="http://purl.obolibrary.org/obo/GAZ_00015352">
        <rdf:type rdf:resource="http://purl.obolibrary.org/obo/ENVO_00000004"/>
        <obo:RO_0001025 rdf:resource="http://purl.obolibrary.org/obo/GAZ_00005376"/>
        <obo:IAO_0000115>A district in southeastern Uganda. Kamuli District is bordered by Kayunga District to the west, Kaberamaido District and Soroti District to the north, across Lake Kyoga. Kaliro District lies to the northeast and Iganga District lies to the southeast of Kamuli District. Directly south of the district lies Jinja District.</obo:IAO_0000115>
        <oboInOwl:hasOBONamespace>GAZ</oboInOwl:hasOBONamespace>
        <oboInOwl:id>GAZ:00015352</oboInOwl:id>
        <rdfs:label>Kamuli District</rdfs:label>
    </owl:NamedIndividual>
    


    <!-- http://purl.obolibrary.org/obo/GAZ_00015353 -->

    <owl:NamedIndividual rdf:about="http://purl.obolibrary.org/obo/GAZ_00015353">
        <rdf:type rdf:resource="http://purl.obolibrary.org/obo/ENVO_00000004"/>
        <obo:RO_0001025 rdf:resource="http://purl.obolibrary.org/obo/GAZ_00236607"/>
        <obo:IAO_0000115>A district in the Eastern Region of Uganda. Amuria District is bordered by Moroto District to the north, Katakwi District to the east, Soroti District to the south, Kaberamaido District to the southwest and Lira District to the west.</obo:IAO_0000115>
        <oboInOwl:hasOBONamespace>GAZ</oboInOwl:hasOBONamespace>
        <oboInOwl:id>GAZ:00015353</oboInOwl:id>
        <rdfs:label>Amuria District</rdfs:label>
    </owl:NamedIndividual>
    


    <!-- http://purl.obolibrary.org/obo/GAZ_00015354 -->

    <owl:NamedIndividual rdf:about="http://purl.obolibrary.org/obo/GAZ_00015354">
        <rdf:type rdf:resource="http://purl.obolibrary.org/obo/ENVO_00000004"/>
        <obo:RO_0001025 rdf:resource="http://purl.obolibrary.org/obo/GAZ_00005376"/>
        <obo:IAO_0000115>A district in eastern Uganda. Busia District borders Busia District, Kenya to the east, Tororo District to the north, Bugiri District to the west and southwest, and Lake Victoria to the south.</obo:IAO_0000115>
        <oboInOwl:hasOBONamespace>GAZ</oboInOwl:hasOBONamespace>
        <oboInOwl:id>GAZ:00015354</oboInOwl:id>
        <rdfs:label>Busia District</rdfs:label>
    </owl:NamedIndividual>
    


    <!-- http://purl.obolibrary.org/obo/GAZ_00015355 -->

    <owl:NamedIndividual rdf:about="http://purl.obolibrary.org/obo/GAZ_00015355">
        <rdf:type rdf:resource="http://purl.obolibrary.org/obo/ENVO_00000004"/>
        <obo:RO_0001025 rdf:resource="http://purl.obolibrary.org/obo/GAZ_00236607"/>
        <obo:IAO_0000115>A district in eastern Uganda. The district is bordered by Amolatar District to the southwest, Dokolo District to the west and northwest, Lira District to the north, Katakwi District to the north east, Soroti District to the east, and Kamuli District across Lake Kyoga to the south.</obo:IAO_0000115>
        <oboInOwl:hasOBONamespace>GAZ</oboInOwl:hasOBONamespace>
        <oboInOwl:id>GAZ:00015355</oboInOwl:id>
        <rdfs:label>Kaberamaido District</rdfs:label>
    </owl:NamedIndividual>
    


    <!-- http://purl.obolibrary.org/obo/GAZ_00015356 -->

    <owl:NamedIndividual rdf:about="http://purl.obolibrary.org/obo/GAZ_00015356">
        <rdf:type rdf:resource="http://purl.obolibrary.org/obo/ENVO_00000004"/>
        <obo:RO_0001025 rdf:resource="http://purl.obolibrary.org/obo/GAZ_00005376"/>
        <obo:IAO_0000115>A district in eastern Uganda. Bukwa District is bordered by Nakapiripirit District in the north, Kapchorwa District to the west, and the Republic of Kenya to the south and east.</obo:IAO_0000115>
        <oboInOwl:hasOBONamespace>GAZ</oboInOwl:hasOBONamespace>
        <oboInOwl:id>GAZ:00015356</oboInOwl:id>
        <rdfs:label>Bukwa District</rdfs:label>
    </owl:NamedIndividual>
    


    <!-- http://purl.obolibrary.org/obo/GAZ_00015357 -->

    <owl:NamedIndividual rdf:about="http://purl.obolibrary.org/obo/GAZ_00015357">
        <rdf:type rdf:resource="http://purl.obolibrary.org/obo/ENVO_00000004"/>
        <obo:RO_0001025 rdf:resource="http://purl.obolibrary.org/obo/GAZ_00236607"/>
        <obo:IAO_0000115>A district in eastern Uganda. Katakwi District is bordered by Moroto District to the north and east, Kumi District to the south and Amuria District to the west.</obo:IAO_0000115>
        <oboInOwl:hasOBONamespace>GAZ</oboInOwl:hasOBONamespace>
        <oboInOwl:id>GAZ:00015357</oboInOwl:id>
        <rdfs:label>Katakwi District</rdfs:label>
    </owl:NamedIndividual>
    


    <!-- http://purl.obolibrary.org/obo/GAZ_00015358 -->

    <owl:NamedIndividual rdf:about="http://purl.obolibrary.org/obo/GAZ_00015358">
        <rdf:type rdf:resource="http://purl.obolibrary.org/obo/ENVO_00000004"/>
        <obo:RO_0001025 rdf:resource="http://purl.obolibrary.org/obo/GAZ_00005376"/>
        <obo:IAO_0000115>A district in eastern Uganda. Iganga District is bordered by Kaliro District to the north, Namutumba District to the northeast, Bugiri District to the east, Mayuge District to the southeast, Jinja District to the southwest and Kamuli District to the west.</obo:IAO_0000115>
        <oboInOwl:hasOBONamespace>GAZ</oboInOwl:hasOBONamespace>
        <oboInOwl:id>GAZ:00015358</oboInOwl:id>
        <rdfs:label>Iganga District</rdfs:label>
    </owl:NamedIndividual>
    


    <!-- http://purl.obolibrary.org/obo/GAZ_00015359 -->

    <owl:NamedIndividual rdf:about="http://purl.obolibrary.org/obo/GAZ_00015359">
        <rdf:type rdf:resource="http://purl.obolibrary.org/obo/ENVO_00000004"/>
        <obo:RO_0001025 rdf:resource="http://purl.obolibrary.org/obo/GAZ_00005376"/>
        <obo:IAO_0000115>A district in the Eastern Region of Uganda. Butaleja District is bordered by Budaka District to the north, Mbale District to the east, Tororo District to the south, Bugiri District to the southwest, Namutumba District to the west, and Pallisa District to the northwest.</obo:IAO_0000115>
        <oboInOwl:hasOBONamespace>GAZ</oboInOwl:hasOBONamespace>
        <oboInOwl:id>GAZ:00015359</oboInOwl:id>
        <rdfs:label>Butaleja District</rdfs:label>
    </owl:NamedIndividual>
    


    <!-- http://purl.obolibrary.org/obo/GAZ_00015360 -->

    <owl:NamedIndividual rdf:about="http://purl.obolibrary.org/obo/GAZ_00015360">
        <rdf:type rdf:resource="http://purl.obolibrary.org/obo/ENVO_00000004"/>
        <obo:RO_0001025 rdf:resource="http://purl.obolibrary.org/obo/GAZ_00005376"/>
        <obo:IAO_0000115>A district in the Eastern Region of Uganda. Kaliro Distict borders Kamuli District in the west, from which it was split. In the north, the district borders Soroti District, across Lake Nakuwa, part of the lakes that comprise the Lake Kyoga water complex. Pallisa District lies to the northeast. Iganga District lies to the southeast and to the south.</obo:IAO_0000115>
        <oboInOwl:hasOBONamespace>GAZ</oboInOwl:hasOBONamespace>
        <oboInOwl:id>GAZ:00015360</oboInOwl:id>
        <rdfs:label>Kaliro District</rdfs:label>
    </owl:NamedIndividual>
    


    <!-- http://purl.obolibrary.org/obo/GAZ_00015361 -->

    <owl:NamedIndividual rdf:about="http://purl.obolibrary.org/obo/GAZ_00015361">
        <rdf:type rdf:resource="http://purl.obolibrary.org/obo/ENVO_00000004"/>
        <obo:RO_0001025 rdf:resource="http://purl.obolibrary.org/obo/GAZ_00005376"/>
        <obo:IAO_0000115>A district in eastern Uganda. It shares borders with the districts of Mbale in the west and south, Nakapiripirit in the north and the Republic of Kenya in the east and south.</obo:IAO_0000115>
        <oboInOwl:hasOBONamespace>GAZ</oboInOwl:hasOBONamespace>
        <oboInOwl:id>GAZ:00015361</oboInOwl:id>
        <rdfs:label>Kapchorwa District</rdfs:label>
    </owl:NamedIndividual>
    


    <!-- http://purl.obolibrary.org/obo/GAZ_00015362 -->

    <owl:NamedIndividual rdf:about="http://purl.obolibrary.org/obo/GAZ_00015362">
        <rdf:type rdf:resource="http://purl.obolibrary.org/obo/ENVO_00000004"/>
        <obo:RO_0001025 rdf:resource="http://purl.obolibrary.org/obo/GAZ_00005376"/>
        <obo:IAO_0000115>A district in eastern Uganda. Bugiri District is bordered by Namutumba District and Butaleja District to the north, Tororo District to the northeast, Busia District to the southeast, the Republic of Tanzania to the south, Mayuge District to the southwest and Iganga District to the west.</obo:IAO_0000115>
        <oboInOwl:hasOBONamespace>GAZ</oboInOwl:hasOBONamespace>
        <oboInOwl:id>GAZ:00015362</oboInOwl:id>
        <rdfs:label>Bugiri District</rdfs:label>
    </owl:NamedIndividual>
    


    <!-- http://purl.obolibrary.org/obo/GAZ_00015363 -->

    <owl:NamedIndividual rdf:about="http://purl.obolibrary.org/obo/GAZ_00015363">
        <rdf:type rdf:resource="http://purl.obolibrary.org/obo/ENVO_00000004"/>
        <obo:RO_0001025 rdf:resource="http://purl.obolibrary.org/obo/GAZ_00005376"/>
        <obo:IAO_0000115>A district in the Eastern Region of Uganda. Namutumba District is bordered by Pallisa District to the north, Butaleja District to the east, Bugiri District to the south, Iganga District to the southwest and Kaliro District to the northwest.</obo:IAO_0000115>
        <oboInOwl:hasOBONamespace>GAZ</oboInOwl:hasOBONamespace>
        <oboInOwl:id>GAZ:00015363</oboInOwl:id>
        <rdfs:label>Namutumba District</rdfs:label>
    </owl:NamedIndividual>
    


    <!-- http://purl.obolibrary.org/obo/GAZ_00015364 -->

    <owl:NamedIndividual rdf:about="http://purl.obolibrary.org/obo/GAZ_00015364">
        <rdf:type rdf:resource="http://purl.obolibrary.org/obo/ENVO_00000004"/>
        <obo:RO_0001025 rdf:resource="http://purl.obolibrary.org/obo/GAZ_00005376"/>
        <obo:IAO_0000115>A district in the Eastern Region of Uganda. Bududa District is bordered by Manafwa District to the south, Mbale District to the west, Sironko District to the north and by the Republic of Kenya to the east.</obo:IAO_0000115>
        <oboInOwl:hasOBONamespace>GAZ</oboInOwl:hasOBONamespace>
        <oboInOwl:id>GAZ:00015364</oboInOwl:id>
        <rdfs:label>Bududa District</rdfs:label>
    </owl:NamedIndividual>
    


    <!-- http://purl.obolibrary.org/obo/GAZ_00015365 -->

    <owl:NamedIndividual rdf:about="http://purl.obolibrary.org/obo/GAZ_00015365">
        <rdf:type rdf:resource="http://purl.obolibrary.org/obo/ENVO_00000004"/>
        <obo:RO_0001025 rdf:resource="http://purl.obolibrary.org/obo/GAZ_00005376"/>
        <obo:IAO_0000115>A district of Uganda created 2005.07-1. Budaka district is located in southeastern Uganda. It is bordered by Kumi District to the north, Mbale District to the east, Butaleja District to the south and Pallisa District to the west.</obo:IAO_0000115>
        <oboInOwl:hasOBONamespace>GAZ</oboInOwl:hasOBONamespace>
        <oboInOwl:id>GAZ:00015365</oboInOwl:id>
        <rdfs:label>Budaka District</rdfs:label>
    </owl:NamedIndividual>
    


    <!-- http://purl.obolibrary.org/obo/GAZ_00015366 -->

    <owl:NamedIndividual rdf:about="http://purl.obolibrary.org/obo/GAZ_00015366">
        <rdf:type rdf:resource="http://purl.obolibrary.org/obo/ENVO_00000004"/>
        <obo:RO_0001025 rdf:resource="http://purl.obolibrary.org/obo/GAZ_00236607"/>
        <obo:IAO_0000115>A district in the Eastern Region of Uganda. Bukedea District is bordered by Katakwi District to the north, Sironko District to the east, Mbale District to the southeast, Budaka District to the south and Kumi District to the west.</obo:IAO_0000115>
        <oboInOwl:hasOBONamespace>GAZ</oboInOwl:hasOBONamespace>
        <oboInOwl:id>GAZ:00015366</oboInOwl:id>
        <rdfs:label>Bukedea District</rdfs:label>
    </owl:NamedIndividual>
    


    <!-- http://purl.obolibrary.org/obo/GAZ_00015367 -->

    <owl:NamedIndividual rdf:about="http://purl.obolibrary.org/obo/GAZ_00015367">
        <rdf:type rdf:resource="http://purl.obolibrary.org/obo/ENVO_00000004"/>
        <obo:RO_0001025 rdf:resource="http://purl.obolibrary.org/obo/GAZ_00005376"/>
        <obo:IAO_0000115>A district in eastern Uganda. Mbale District is bordered by Tororo District in the south, Manafwa District in the southeast, Sironko District in the northeast, Kumi District in the north, Budaka District in the northwest and Butaleja District in the southwest.</obo:IAO_0000115>
        <oboInOwl:hasOBONamespace>GAZ</oboInOwl:hasOBONamespace>
        <oboInOwl:id>GAZ:00015367</oboInOwl:id>
        <rdfs:label>Mbale District</rdfs:label>
    </owl:NamedIndividual>
    


    <!-- http://purl.obolibrary.org/obo/GAZ_00015368 -->

    <owl:NamedIndividual rdf:about="http://purl.obolibrary.org/obo/GAZ_00015368">
        <rdf:type rdf:resource="http://purl.obolibrary.org/obo/ENVO_00000004"/>
        <obo:RO_0001025 rdf:resource="http://purl.obolibrary.org/obo/GAZ_00236607"/>
        <obo:IAO_0000115>A district in eastern Uganda. Kumi District is bordered by Mbale District to the southeast, Sironko District to the east, Nakapiripirit District and Moroto District to the northeast, Katakwi District to the north, Amuria District to the northeast, Soroti District to the west, Pallisa District and Budaka District to the south.</obo:IAO_0000115>
        <oboInOwl:hasOBONamespace>GAZ</oboInOwl:hasOBONamespace>
        <oboInOwl:id>GAZ:00015368</oboInOwl:id>
        <rdfs:label>Kumi District</rdfs:label>
    </owl:NamedIndividual>
    


    <!-- http://purl.obolibrary.org/obo/GAZ_00015369 -->

    <owl:NamedIndividual rdf:about="http://purl.obolibrary.org/obo/GAZ_00015369">
        <rdf:type rdf:resource="http://purl.obolibrary.org/obo/ENVO_00000004"/>
        <obo:RO_0001025 rdf:resource="http://purl.obolibrary.org/obo/GAZ_00005376"/>
        <obo:IAO_0000115>A district in eastern Uganda. Sironko District is bordered by Manafwa District to the south, Mbale District to the southwest, Kumi District to the west, Nakapiripirit District to the north, Kapchorwa District to the east and Kenya to the southeast.</obo:IAO_0000115>
        <oboInOwl:hasOBONamespace>GAZ</oboInOwl:hasOBONamespace>
        <oboInOwl:id>GAZ:00015369</oboInOwl:id>
        <rdfs:label>Sironko District</rdfs:label>
    </owl:NamedIndividual>
    


    <!-- http://purl.obolibrary.org/obo/GAZ_00015370 -->

    <owl:NamedIndividual rdf:about="http://purl.obolibrary.org/obo/GAZ_00015370">
        <rdf:type rdf:resource="http://purl.obolibrary.org/obo/ENVO_00000004"/>
        <obo:RO_0001025 rdf:resource="http://purl.obolibrary.org/obo/GAZ_00005376"/>
        <obo:IAO_0000115>A district in eastern Uganda. Pallisa District is bordered by Kumi District to the north, Budaka District to the east, Butaleja District to the southeast, Namutumba District to the south, Kaliro District to the west, to the northwest lies both Kamuli District and Soroti District.</obo:IAO_0000115>
        <oboInOwl:hasOBONamespace>GAZ</oboInOwl:hasOBONamespace>
        <oboInOwl:id>GAZ:00015370</oboInOwl:id>
        <rdfs:label>Pallisa District</rdfs:label>
    </owl:NamedIndividual>
    


    <!-- http://purl.obolibrary.org/obo/GAZ_00015371 -->

    <owl:NamedIndividual rdf:about="http://purl.obolibrary.org/obo/GAZ_00015371">
        <rdf:type rdf:resource="http://purl.obolibrary.org/obo/ENVO_00000004"/>
        <obo:RO_0001025 rdf:resource="http://purl.obolibrary.org/obo/GAZ_00005376"/>
        <obo:IAO_0000115>A district in eastern Uganda. Tororo District is bordered by the country of Kenya to the east, Busia District to the south, Bugiri District to the southwest, Iganga District to the west, Pallisa District to the north and Mbale District to the northeast.</obo:IAO_0000115>
        <oboInOwl:hasOBONamespace>GAZ</oboInOwl:hasOBONamespace>
        <oboInOwl:id>GAZ:00015371</oboInOwl:id>
        <rdfs:label>Tororo District</rdfs:label>
    </owl:NamedIndividual>
    


    <!-- http://purl.obolibrary.org/obo/GAZ_00015372 -->

    <owl:NamedIndividual rdf:about="http://purl.obolibrary.org/obo/GAZ_00015372">
        <rdf:type rdf:resource="http://purl.obolibrary.org/obo/ENVO_00000004"/>
        <obo:RO_0001025 rdf:resource="http://purl.obolibrary.org/obo/GAZ_00236607"/>
        <obo:IAO_0000115>A district in eastern Uganda. Soroti District is bordered by Kumi District to the east, Amuria District to the north, Kaberamaido District to the west, Kamuli District to the southwest, Kaliro District to the south and Pallisa District to the southeast.</obo:IAO_0000115>
        <oboInOwl:hasOBONamespace>GAZ</oboInOwl:hasOBONamespace>
        <oboInOwl:id>GAZ:00015372</oboInOwl:id>
        <rdfs:label>Soroti District</rdfs:label>
    </owl:NamedIndividual>
    


    <!-- http://purl.obolibrary.org/obo/GAZ_00015373 -->

    <owl:NamedIndividual rdf:about="http://purl.obolibrary.org/obo/GAZ_00015373">
        <rdf:type rdf:resource="http://purl.obolibrary.org/obo/ENVO_00000004"/>
        <obo:RO_0001025 rdf:resource="http://purl.obolibrary.org/obo/GAZ_00005376"/>
        <obo:IAO_0000115>A district in the Eastern Region of Uganda. Manafwa is bordered by Tororo District to the south, Mbale District to the west, Bududa District to the north and by the Republic of Kenya to the east.</obo:IAO_0000115>
        <oboInOwl:hasOBONamespace>GAZ</oboInOwl:hasOBONamespace>
        <oboInOwl:id>GAZ:00015373</oboInOwl:id>
        <rdfs:label>Manafwa District</rdfs:label>
    </owl:NamedIndividual>
    


    <!-- http://purl.obolibrary.org/obo/GAZ_00015374 -->

    <owl:NamedIndividual rdf:about="http://purl.obolibrary.org/obo/GAZ_00015374">
        <rdf:type rdf:resource="http://purl.obolibrary.org/obo/ENVO_00000004"/>
        <obo:RO_0001025 rdf:resource="http://purl.obolibrary.org/obo/GAZ_00005376"/>
        <obo:IAO_0000115>A district in eastern Uganda. Mayuge District is bordered by Iganga District to the north, Bugiri District to the northeast and east, the Republic of Tanzania to the south, Mukono District to the southwest and Jinja District to the west.</obo:IAO_0000115>
        <oboInOwl:hasOBONamespace>GAZ</oboInOwl:hasOBONamespace>
        <oboInOwl:id>GAZ:00015374</oboInOwl:id>
        <rdfs:label>Mayuge District</rdfs:label>
    </owl:NamedIndividual>
    


    <!-- http://purl.obolibrary.org/obo/GAZ_00015375 -->

    <owl:NamedIndividual rdf:about="http://purl.obolibrary.org/obo/GAZ_00015375">
        <rdf:type rdf:resource="http://purl.obolibrary.org/obo/ENVO_00000004"/>
        <obo:RO_0001025 rdf:resource="http://purl.obolibrary.org/obo/GAZ_00236608"/>
        <obo:IAO_0000115>A district in north-western Uganda. Nebbi District is bordered by Arua District to the north, Amuru District to the east, Bulisa District to the southeast and the Democratic Republic of the Congo (DRC) to the south and west.</obo:IAO_0000115>
        <oboInOwl:hasOBONamespace>GAZ</oboInOwl:hasOBONamespace>
        <oboInOwl:id>GAZ:00015375</oboInOwl:id>
        <rdfs:label>Nebbi District</rdfs:label>
    </owl:NamedIndividual>
    


    <!-- http://purl.obolibrary.org/obo/GAZ_00015376 -->

    <owl:NamedIndividual rdf:about="http://purl.obolibrary.org/obo/GAZ_00015376">
        <rdf:type rdf:resource="http://purl.obolibrary.org/obo/ENVO_00000004"/>
        <obo:RO_0001025 rdf:resource="http://purl.obolibrary.org/obo/GAZ_00236608"/>
        <obo:IAO_0000115>A district in West Nile, in northern Uganda. Yumbe District is one of Uganda&apos;s most northern districts. The district is bordered by Southern Sudan to the north, Moyo District to the east, Adjumani District and Arua District to the southeast, Maracha-Terego District to the south and Koboko District to the west.</obo:IAO_0000115>
        <oboInOwl:hasOBONamespace>GAZ</oboInOwl:hasOBONamespace>
        <oboInOwl:id>GAZ:00015376</oboInOwl:id>
        <rdfs:label>Yumbe District</rdfs:label>
    </owl:NamedIndividual>
    


    <!-- http://purl.obolibrary.org/obo/GAZ_00015377 -->

    <owl:NamedIndividual rdf:about="http://purl.obolibrary.org/obo/GAZ_00015377">
        <rdf:type rdf:resource="http://purl.obolibrary.org/obo/ENVO_00000004"/>
        <obo:RO_0001025 rdf:resource="http://purl.obolibrary.org/obo/GAZ_00233544"/>
        <obo:IAO_0000115>A district in the Northern Region of Uganda. Kotido District is bordered by Kaabong District to the north, Moroto District to the east and south, Abim District to the west, Pader District and Kitgum District to the northwest.</obo:IAO_0000115>
        <oboInOwl:hasOBONamespace>GAZ</oboInOwl:hasOBONamespace>
        <oboInOwl:id>GAZ:00015377</oboInOwl:id>
        <rdfs:label>Kotido District</rdfs:label>
    </owl:NamedIndividual>
    


    <!-- http://purl.obolibrary.org/obo/GAZ_00015378 -->

    <owl:NamedIndividual rdf:about="http://purl.obolibrary.org/obo/GAZ_00015378">
        <rdf:type rdf:resource="http://purl.obolibrary.org/obo/ENVO_00000004"/>
        <obo:RO_0001025 rdf:resource="http://purl.obolibrary.org/obo/GAZ_00236609"/>
        <obo:IAO_0000115>A district in Lango sub-region in northern Uganda. Lira District is bordered by Dokolo District to the south, Amuria District to the east, Moroto District and Abim District to the northeast, Pader District to the north, Oyam District to the northwest and Apac District to the west.</obo:IAO_0000115>
        <oboInOwl:hasOBONamespace>GAZ</oboInOwl:hasOBONamespace>
        <oboInOwl:id>GAZ:00015378</oboInOwl:id>
        <rdfs:label>Lira District</rdfs:label>
    </owl:NamedIndividual>
    


    <!-- http://purl.obolibrary.org/obo/GAZ_00015379 -->

    <owl:NamedIndividual rdf:about="http://purl.obolibrary.org/obo/GAZ_00015379">
        <rdf:type rdf:resource="http://purl.obolibrary.org/obo/ENVO_00000004"/>
        <obo:RO_0001025 rdf:resource="http://purl.obolibrary.org/obo/GAZ_00005375"/>
        <obo:IAO_0000115>A district in the Northern Region of Uganda. Oyam District is bordered by Gulu District to the north, Pader District and Lira District to the northeast, Apac District to the east and south, Masindi District to the southwest and Amuru District to the west.</obo:IAO_0000115>
        <oboInOwl:hasOBONamespace>GAZ</oboInOwl:hasOBONamespace>
        <oboInOwl:id>GAZ:00015379</oboInOwl:id>
        <rdfs:label>Oyam District</rdfs:label>
    </owl:NamedIndividual>
    


    <!-- http://purl.obolibrary.org/obo/GAZ_00015380 -->

    <owl:NamedIndividual rdf:about="http://purl.obolibrary.org/obo/GAZ_00015380">
        <rdf:type rdf:resource="http://purl.obolibrary.org/obo/ENVO_00000004"/>
        <obo:RO_0001025 rdf:resource="http://purl.obolibrary.org/obo/GAZ_00236917"/>
        <obo:IAO_0000115>A district in northern Uganda. Kitgum District is bordered by Southern Sudan to the north, Kaabong District to the east, Kotido District to the southeast, Pader District to the south, Gulu District to the southwest and Amuru District to the west.</obo:IAO_0000115>
        <oboInOwl:hasOBONamespace>GAZ</oboInOwl:hasOBONamespace>
        <oboInOwl:id>GAZ:00015380</oboInOwl:id>
        <rdfs:label>Kitgum District</rdfs:label>
    </owl:NamedIndividual>
    


    <!-- http://purl.obolibrary.org/obo/GAZ_00015381 -->

    <owl:NamedIndividual rdf:about="http://purl.obolibrary.org/obo/GAZ_00015381">
        <rdf:type rdf:resource="http://purl.obolibrary.org/obo/ENVO_00000004"/>
        <obo:RO_0001025 rdf:resource="http://purl.obolibrary.org/obo/GAZ_00236917"/>
        <obo:IAO_0000115>A district in northern Uganda.</obo:IAO_0000115>
        <oboInOwl:hasOBONamespace>GAZ</oboInOwl:hasOBONamespace>
        <oboInOwl:id>GAZ:00015381</oboInOwl:id>
        <rdfs:label>Pader District</rdfs:label>
    </owl:NamedIndividual>
    


    <!-- http://purl.obolibrary.org/obo/GAZ_00015382 -->

    <owl:NamedIndividual rdf:about="http://purl.obolibrary.org/obo/GAZ_00015382">
        <rdf:type rdf:resource="http://purl.obolibrary.org/obo/ENVO_00000004"/>
        <obo:RO_0001025 rdf:resource="http://purl.obolibrary.org/obo/GAZ_00233544"/>
        <obo:IAO_0000115>A district in the Northern Region of Uganda. Kaabong District is bordered by Southern Sudan to the northwest, the Republic of Kenya to the northeast, and the east, Moroto District to the southeast, Kotido District to the south and Kitgum District to the west.</obo:IAO_0000115>
        <oboInOwl:hasOBONamespace>GAZ</oboInOwl:hasOBONamespace>
        <oboInOwl:id>GAZ:00015382</oboInOwl:id>
        <rdfs:label>Kaabong District</rdfs:label>
    </owl:NamedIndividual>
    


    <!-- http://purl.obolibrary.org/obo/GAZ_00015383 -->

    <owl:NamedIndividual rdf:about="http://purl.obolibrary.org/obo/GAZ_00015383">
        <rdf:type rdf:resource="http://purl.obolibrary.org/obo/ENVO_00000004"/>
        <obo:RO_0001025 rdf:resource="http://purl.obolibrary.org/obo/GAZ_00233544"/>
        <obo:IAO_0000115>A district in northeastern Uganda. The district is bordered to the south by three districts, namely; Sironko, Kapchorwa and Bukwa. Kenya lies to the east, Moroto District lies to the north and Kumi District lies to the west.</obo:IAO_0000115>
        <oboInOwl:hasOBONamespace>GAZ</oboInOwl:hasOBONamespace>
        <oboInOwl:id>GAZ:00015383</oboInOwl:id>
        <rdfs:label>Nakapiripirit District</rdfs:label>
    </owl:NamedIndividual>
    


    <!-- http://purl.obolibrary.org/obo/GAZ_00015384 -->

    <owl:NamedIndividual rdf:about="http://purl.obolibrary.org/obo/GAZ_00015384">
        <rdf:type rdf:resource="http://purl.obolibrary.org/obo/ENVO_00000004"/>
        <obo:RO_0001025 rdf:resource="http://purl.obolibrary.org/obo/GAZ_00236609"/>
        <obo:IAO_0000115>A district in the Northern Region of Uganda. Dokolo District is bordered by Lira District to the north, Amuria District to the northeast, Kaberamaido District to the east and south, Amolatar District to the southwest and Apac District to the west.</obo:IAO_0000115>
        <oboInOwl:hasOBONamespace>GAZ</oboInOwl:hasOBONamespace>
        <oboInOwl:id>GAZ:00015384</oboInOwl:id>
        <rdfs:label>Dokolo District</rdfs:label>
    </owl:NamedIndividual>
    


    <!-- http://purl.obolibrary.org/obo/GAZ_00015385 -->

    <owl:NamedIndividual rdf:about="http://purl.obolibrary.org/obo/GAZ_00015385">
        <rdf:type rdf:resource="http://purl.obolibrary.org/obo/ENVO_00000004"/>
        <obo:RO_0001025 rdf:resource="http://purl.obolibrary.org/obo/GAZ_00236608"/>
        <obo:IAO_0000115>A district in northern Uganda. Moyo District is bordered by Southern Sudan to the north, Adjumani District to the south, across the waters of the White Nile, and Yumbe District to the west.</obo:IAO_0000115>
        <oboInOwl:hasOBONamespace>GAZ</oboInOwl:hasOBONamespace>
        <oboInOwl:id>GAZ:00015385</oboInOwl:id>
        <rdfs:label>Moyo District</rdfs:label>
    </owl:NamedIndividual>
    


    <!-- http://purl.obolibrary.org/obo/GAZ_00015386 -->

    <owl:NamedIndividual rdf:about="http://purl.obolibrary.org/obo/GAZ_00015386">
        <obo:RO_0001025 rdf:resource="http://purl.obolibrary.org/obo/GAZ_00005375"/>
        <obo:IAO_0000115>A District of the Northern Region of Uganda.</obo:IAO_0000115>
        <oboInOwl:hasOBONamespace>GAZ</oboInOwl:hasOBONamespace>
        <oboInOwl:id>GAZ:00015386</oboInOwl:id>
        <rdfs:label>Maracha-Terego District</rdfs:label>
    </owl:NamedIndividual>
    


    <!-- http://purl.obolibrary.org/obo/GAZ_00015387 -->

    <owl:NamedIndividual rdf:about="http://purl.obolibrary.org/obo/GAZ_00015387">
        <rdf:type rdf:resource="http://purl.obolibrary.org/obo/ENVO_00000004"/>
        <obo:RO_0001025 rdf:resource="http://purl.obolibrary.org/obo/GAZ_00236608"/>
        <obo:IAO_0000115>A district of Uganda located in the northwestern corner of the country. Koboko District is bordered by Southern Sudan to the north, Yumbe District to the east, Maracha-Terego District to the south and the Democratic Republic of the Congo to the west.</obo:IAO_0000115>
        <oboInOwl:hasOBONamespace>GAZ</oboInOwl:hasOBONamespace>
        <oboInOwl:id>GAZ:00015387</oboInOwl:id>
        <rdfs:label>Koboko District</rdfs:label>
    </owl:NamedIndividual>
    


    <!-- http://purl.obolibrary.org/obo/GAZ_00015388 -->

    <owl:NamedIndividual rdf:about="http://purl.obolibrary.org/obo/GAZ_00015388">
        <rdf:type rdf:resource="http://purl.obolibrary.org/obo/ENVO_00000004"/>
        <obo:RO_0001025 rdf:resource="http://purl.obolibrary.org/obo/GAZ_00236609"/>
        <obo:IAO_0000115>A district in the Northern Region of Uganda. Amolatar District is bordered by Apac District to the north, Dokolo District to the northeast, Kaberamaido District to the east, Kamuli District to the southeast, Kayunga District to the south and Nakasongola District to the southwest and west.</obo:IAO_0000115>
        <oboInOwl:hasOBONamespace>GAZ</oboInOwl:hasOBONamespace>
        <oboInOwl:id>GAZ:00015388</oboInOwl:id>
        <rdfs:label>Amolatar District</rdfs:label>
    </owl:NamedIndividual>
    


    <!-- http://purl.obolibrary.org/obo/GAZ_00015389 -->

    <owl:NamedIndividual rdf:about="http://purl.obolibrary.org/obo/GAZ_00015389">
        <rdf:type rdf:resource="http://purl.obolibrary.org/obo/ENVO_00000004"/>
        <obo:RO_0001025 rdf:resource="http://purl.obolibrary.org/obo/GAZ_00236608"/>
        <obo:IAO_0000115>A district in northwestern Uganda. Arua District is bordered by Nebbi District to the south, Amuru District to the east, Adjumani District to the northeast, Maracha-Terego District to the north and the Democratic Republic of the Congo to the west.</obo:IAO_0000115>
        <oboInOwl:hasOBONamespace>GAZ</oboInOwl:hasOBONamespace>
        <oboInOwl:id>GAZ:00015389</oboInOwl:id>
        <rdfs:label>Arua District</rdfs:label>
    </owl:NamedIndividual>
    


    <!-- http://purl.obolibrary.org/obo/GAZ_00015390 -->

    <owl:NamedIndividual rdf:about="http://purl.obolibrary.org/obo/GAZ_00015390">
        <rdf:type rdf:resource="http://purl.obolibrary.org/obo/ENVO_00000004"/>
        <obo:RO_0001025 rdf:resource="http://purl.obolibrary.org/obo/GAZ_00005375"/>
        <obo:IAO_0000115>A district in northern Uganda. Adjumani District is bordered by Moyo District to the north, Southern Sudan to the northeast, Amuru District to the east and south, Arua District to the southwest and Yumbe District to the northwest.</obo:IAO_0000115>
        <oboInOwl:hasOBONamespace>GAZ</oboInOwl:hasOBONamespace>
        <oboInOwl:id>GAZ:00015390</oboInOwl:id>
        <rdfs:label>Adjumani District</rdfs:label>
    </owl:NamedIndividual>
    


    <!-- http://purl.obolibrary.org/obo/GAZ_00015391 -->

    <owl:NamedIndividual rdf:about="http://purl.obolibrary.org/obo/GAZ_00015391">
        <rdf:type rdf:resource="http://purl.obolibrary.org/obo/ENVO_00000004"/>
        <obo:RO_0001025 rdf:resource="http://purl.obolibrary.org/obo/GAZ_00236917"/>
        <obo:IAO_0000115>A district in the Northern Region of Uganda. It is bordered by Adjumani District to the north, Southern Sudan and Kitgum District to the northeast, Gulu District to the east, Oyam District to the southeast, Masindi District and Bulisa District to the south, Nebbi District to the west and Arua District to the northwest.</obo:IAO_0000115>
        <oboInOwl:hasOBONamespace>GAZ</oboInOwl:hasOBONamespace>
        <oboInOwl:id>GAZ:00015391</oboInOwl:id>
        <rdfs:label>Amuru District</rdfs:label>
    </owl:NamedIndividual>
    


    <!-- http://purl.obolibrary.org/obo/GAZ_00015392 -->

    <owl:NamedIndividual rdf:about="http://purl.obolibrary.org/obo/GAZ_00015392">
        <rdf:type rdf:resource="http://purl.obolibrary.org/obo/ENVO_00000004"/>
        <obo:RO_0001025 rdf:resource="http://purl.obolibrary.org/obo/GAZ_00233544"/>
        <obo:IAO_0000115>A district in the Northern Region of Uganda. Abim District is bordered by Kotido District to the north and east, Moroto District to the southeast and south, Lira District to the southwest and Pader District to the west.</obo:IAO_0000115>
        <oboInOwl:hasOBONamespace>GAZ</oboInOwl:hasOBONamespace>
        <oboInOwl:id>GAZ:00015392</oboInOwl:id>
        <rdfs:label>Abim District</rdfs:label>
    </owl:NamedIndividual>
    


    <!-- http://purl.obolibrary.org/obo/GAZ_00015393 -->

    <owl:NamedIndividual rdf:about="http://purl.obolibrary.org/obo/GAZ_00015393">
        <rdf:type rdf:resource="http://purl.obolibrary.org/obo/ENVO_00000004"/>
        <obo:RO_0001025 rdf:resource="http://purl.obolibrary.org/obo/GAZ_00236609"/>
        <obo:IAO_0000115>A district in northern Uganda. Apac District is ordered by Oyam District to the northwest, Lira District to the northeast, Dokolo District to the southeast, Amolatar District to the south, Nakasongola District to the southwest and Masindi District to the west.</obo:IAO_0000115>
        <oboInOwl:hasOBONamespace>GAZ</oboInOwl:hasOBONamespace>
        <oboInOwl:id>GAZ:00015393</oboInOwl:id>
        <rdfs:label>Apac District</rdfs:label>
    </owl:NamedIndividual>
    


    <!-- http://purl.obolibrary.org/obo/GAZ_00015394 -->

    <owl:NamedIndividual rdf:about="http://purl.obolibrary.org/obo/GAZ_00015394">
        <rdf:type rdf:resource="http://purl.obolibrary.org/obo/ENVO_00000004"/>
        <obo:RO_0001025 rdf:resource="http://purl.obolibrary.org/obo/GAZ_00005374"/>
        <obo:IAO_0000115>A district in western Uganda. Kasese District is located along the Equator. It is bordered by Kabarole District to the north, Kamwenge District to the east, Bushenyi District to the south and the Democratic Republic of the Congo to the west.</obo:IAO_0000115>
        <oboInOwl:hasOBONamespace>GAZ</oboInOwl:hasOBONamespace>
        <oboInOwl:id>GAZ:00015394</oboInOwl:id>
        <rdfs:label>Kasese District</rdfs:label>
    </owl:NamedIndividual>
    


    <!-- http://purl.obolibrary.org/obo/GAZ_00015395 -->

    <owl:NamedIndividual rdf:about="http://purl.obolibrary.org/obo/GAZ_00015395">
        <rdf:type rdf:resource="http://purl.obolibrary.org/obo/ENVO_00000004"/>
        <obo:RO_0001025 rdf:resource="http://purl.obolibrary.org/obo/GAZ_00005374"/>
        <obo:IAO_0000115>A district in western Uganda. Bulisa District is bordered by Amuru District to the north, Masindi District to the east and south, Hoima District to the southwest and the Democratic Republic of the Congo to the west.</obo:IAO_0000115>
        <oboInOwl:hasOBONamespace>GAZ</oboInOwl:hasOBONamespace>
        <oboInOwl:id>GAZ:00015395</oboInOwl:id>
        <rdfs:label>Bulisa District</rdfs:label>
    </owl:NamedIndividual>
    


    <!-- http://purl.obolibrary.org/obo/GAZ_00015396 -->

    <owl:NamedIndividual rdf:about="http://purl.obolibrary.org/obo/GAZ_00015396">
        <rdf:type rdf:resource="http://purl.obolibrary.org/obo/ENVO_00000004"/>
        <obo:RO_0001025 rdf:resource="http://purl.obolibrary.org/obo/GAZ_00005374"/>
        <obo:IAO_0000115>A district in western Uganda. The district is bordered by Kyenjojo District to the east, Kamwenge District to the southeast, Kasese District to the south, the Democratic Republic of the Congo to the southwest and Bundibugyo District to the west and to the north.</obo:IAO_0000115>
        <oboInOwl:hasOBONamespace>GAZ</oboInOwl:hasOBONamespace>
        <oboInOwl:id>GAZ:00015396</oboInOwl:id>
        <rdfs:label>Kabarole District</rdfs:label>
    </owl:NamedIndividual>
    


    <!-- http://purl.obolibrary.org/obo/GAZ_00015397 -->

    <owl:NamedIndividual rdf:about="http://purl.obolibrary.org/obo/GAZ_00015397">
        <rdf:type rdf:resource="http://purl.obolibrary.org/obo/ENVO_00000004"/>
        <obo:RO_0001025 rdf:resource="http://purl.obolibrary.org/obo/GAZ_00005374"/>
        <obo:IAO_0000115>A district in southwestern Uganda. Kabale District is bordered by Ntungamo District to the northeast, Rukungiri District to the north, Kanungu District to the northwest, Kisoro District to the west and the country of Rwanda to the south.</obo:IAO_0000115>
        <oboInOwl:hasOBONamespace>GAZ</oboInOwl:hasOBONamespace>
        <oboInOwl:id>GAZ:00015397</oboInOwl:id>
        <rdfs:label>Kabale District</rdfs:label>
    </owl:NamedIndividual>
    


    <!-- http://purl.obolibrary.org/obo/GAZ_00015398 -->

    <owl:NamedIndividual rdf:about="http://purl.obolibrary.org/obo/GAZ_00015398">
        <rdf:type rdf:resource="http://purl.obolibrary.org/obo/ENVO_00000004"/>
        <obo:RO_0001025 rdf:resource="http://purl.obolibrary.org/obo/GAZ_00005374"/>
        <obo:IAO_0000115>A district in western Uganda. Ibanda District is bordered by Kamwenge District to the northwest and north, Kiruhura District to the east, Mbarara District to the south and Bushenyi District to the southwest.</obo:IAO_0000115>
        <oboInOwl:hasOBONamespace>GAZ</oboInOwl:hasOBONamespace>
        <oboInOwl:id>GAZ:00015398</oboInOwl:id>
        <rdfs:label>Ibanda District</rdfs:label>
    </owl:NamedIndividual>
    


    <!-- http://purl.obolibrary.org/obo/GAZ_00015399 -->

    <owl:NamedIndividual rdf:about="http://purl.obolibrary.org/obo/GAZ_00015399">
        <rdf:type rdf:resource="http://purl.obolibrary.org/obo/ENVO_00000004"/>
        <obo:RO_0001025 rdf:resource="http://purl.obolibrary.org/obo/GAZ_00005374"/>
        <obo:IAO_0000115>A district in southwestern Uganda. Isingiro District is bordered by Rakai District to the east, Kiruhura District to the north, Mbarara District to the northwest, Ntungamo District to the west and the country of Tanzania to the south.</obo:IAO_0000115>
        <oboInOwl:hasOBONamespace>GAZ</oboInOwl:hasOBONamespace>
        <oboInOwl:id>GAZ:00015399</oboInOwl:id>
        <rdfs:label>Isingiro District</rdfs:label>
    </owl:NamedIndividual>
    


    <!-- http://purl.obolibrary.org/obo/GAZ_00015400 -->

    <owl:NamedIndividual rdf:about="http://purl.obolibrary.org/obo/GAZ_00015400">
        <rdf:type rdf:resource="http://purl.obolibrary.org/obo/ENVO_00000004"/>
        <obo:RO_0001025 rdf:resource="http://purl.obolibrary.org/obo/GAZ_00005374"/>
        <obo:IAO_0000115>A district in western Uganda. Hoima District is bordered by Kibale District in the south, Kiboga District in the southeast, Masindi District in the east and northeast, Lake Albert and the Democratic Republic of the Congo in the north and west.</obo:IAO_0000115>
        <oboInOwl:hasOBONamespace>GAZ</oboInOwl:hasOBONamespace>
        <oboInOwl:id>GAZ:00015400</oboInOwl:id>
        <rdfs:label>Hoima District</rdfs:label>
    </owl:NamedIndividual>
    


    <!-- http://purl.obolibrary.org/obo/GAZ_00015401 -->

    <owl:NamedIndividual rdf:about="http://purl.obolibrary.org/obo/GAZ_00015401">
        <rdf:type rdf:resource="http://purl.obolibrary.org/obo/ENVO_00000004"/>
        <obo:RO_0001025 rdf:resource="http://purl.obolibrary.org/obo/GAZ_00005374"/>
        <obo:IAO_0000115>A district in western Uganda. Kibaale District is bordered by Hoima District to the north, Kiboga District to the northeast, Mubende District to the southeast, Kyenjojo District to the south, Kabarole District to the southwest and Bundibugyo District, across Lake Albert to the west.</obo:IAO_0000115>
        <oboInOwl:hasOBONamespace>GAZ</oboInOwl:hasOBONamespace>
        <oboInOwl:id>GAZ:00015401</oboInOwl:id>
        <rdfs:label>Kibaale District</rdfs:label>
    </owl:NamedIndividual>
    


    <!-- http://purl.obolibrary.org/obo/GAZ_00015402 -->

    <owl:NamedIndividual rdf:about="http://purl.obolibrary.org/obo/GAZ_00015402">
        <rdf:type rdf:resource="http://purl.obolibrary.org/obo/ENVO_00000004"/>
        <obo:RO_0001025 rdf:resource="http://purl.obolibrary.org/obo/GAZ_00005374"/>
        <obo:IAO_0000115>A district in western Uganda. Bundibugyo District is bordered by Hoima District to the northeast, Kibale District to the east, Kabarole District to the south, and the Democratic Republic of the Congo to the west and north.</obo:IAO_0000115>
        <oboInOwl:hasOBONamespace>GAZ</oboInOwl:hasOBONamespace>
        <oboInOwl:id>GAZ:00015402</oboInOwl:id>
        <rdfs:label>Bundibugyo District</rdfs:label>
    </owl:NamedIndividual>
    


    <!-- http://purl.obolibrary.org/obo/GAZ_00015403 -->

    <owl:NamedIndividual rdf:about="http://purl.obolibrary.org/obo/GAZ_00015403">
        <rdf:type rdf:resource="http://purl.obolibrary.org/obo/ENVO_00000004"/>
        <obo:RO_0001025 rdf:resource="http://purl.obolibrary.org/obo/GAZ_00005374"/>
        <obo:IAO_0000115>A district in western Uganda. Kamwenge District is bordered by Kabarole District to the north, Kyenjojo District to the northeast, Kiruhura District to the southeast, Ibanda District to the south, Bushenyi District to the southwest and Kasese District to the west.</obo:IAO_0000115>
        <oboInOwl:hasOBONamespace>GAZ</oboInOwl:hasOBONamespace>
        <oboInOwl:id>GAZ:00015403</oboInOwl:id>
        <rdfs:label>Kamwenge District</rdfs:label>
    </owl:NamedIndividual>
    


    <!-- http://purl.obolibrary.org/obo/GAZ_00015404 -->

    <owl:NamedIndividual rdf:about="http://purl.obolibrary.org/obo/GAZ_00015404">
        <rdf:type rdf:resource="http://purl.obolibrary.org/obo/ENVO_00000004"/>
        <obo:RO_0001025 rdf:resource="http://purl.obolibrary.org/obo/GAZ_00005374"/>
        <obo:IAO_0000115>A district in western Uganda. Kanungu District is bordered by Rukungiri District to the north and east, Kabale District to the southeast, Kisoro District to the southwest and the Democratic Republic of the Congo to the west.</obo:IAO_0000115>
        <oboInOwl:hasOBONamespace>GAZ</oboInOwl:hasOBONamespace>
        <oboInOwl:id>GAZ:00015404</oboInOwl:id>
        <rdfs:label>Kanungu District</rdfs:label>
    </owl:NamedIndividual>
    


    <!-- http://purl.obolibrary.org/obo/GAZ_00015405 -->

    <owl:NamedIndividual rdf:about="http://purl.obolibrary.org/obo/GAZ_00015405">
        <rdf:type rdf:resource="http://purl.obolibrary.org/obo/ENVO_00000004"/>
        <obo:RO_0001025 rdf:resource="http://purl.obolibrary.org/obo/GAZ_00005374"/>
        <obo:IAO_0000115>A district in western Uganda. Bushenyi District is bordered by Kasese District to the north, Kamwenge District and Ibanda District to the northeast, Mbarara District to the east, Ntungamo District to the south, Rukungiri District to the southwest and the Democratic Republic of the Congo to the west.</obo:IAO_0000115>
        <oboInOwl:hasOBONamespace>GAZ</oboInOwl:hasOBONamespace>
        <oboInOwl:id>GAZ:00015405</oboInOwl:id>
        <rdfs:label>Bushenyi District</rdfs:label>
    </owl:NamedIndividual>
    


    <!-- http://purl.obolibrary.org/obo/GAZ_00015406 -->

    <owl:NamedIndividual rdf:about="http://purl.obolibrary.org/obo/GAZ_00015406">
        <rdf:type rdf:resource="http://purl.obolibrary.org/obo/ENVO_00000004"/>
        <obo:RO_0001025 rdf:resource="http://purl.obolibrary.org/obo/GAZ_00005374"/>
        <obo:IAO_0000115>A district in western Uganda. Kyenjojo District is bordered by Kibale District to the north, Mubende District to the east, Kiruhura District to the southeast, Kamwenge District to the south and Kabarole District to the west.</obo:IAO_0000115>
        <oboInOwl:hasOBONamespace>GAZ</oboInOwl:hasOBONamespace>
        <oboInOwl:id>GAZ:00015406</oboInOwl:id>
        <rdfs:label>Kyenjojo District</rdfs:label>
    </owl:NamedIndividual>
    


    <!-- http://purl.obolibrary.org/obo/GAZ_00015407 -->

    <owl:NamedIndividual rdf:about="http://purl.obolibrary.org/obo/GAZ_00015407">
        <rdf:type rdf:resource="http://purl.obolibrary.org/obo/ENVO_00000004"/>
        <obo:RO_0001025 rdf:resource="http://purl.obolibrary.org/obo/GAZ_00005374"/>
        <obo:IAO_0000115>A district in the Western Region of Uganda. Kiruhura District is bordered by Rakai District to the east, Sembabule District to the northeast, Kyenjojo District to the north, Mbarara District to the west and Isingiro District to the south.</obo:IAO_0000115>
        <oboInOwl:hasOBONamespace>GAZ</oboInOwl:hasOBONamespace>
        <oboInOwl:id>GAZ:00015407</oboInOwl:id>
        <rdfs:label>Kiruhura District</rdfs:label>
    </owl:NamedIndividual>
    


    <!-- http://purl.obolibrary.org/obo/GAZ_00015408 -->

    <owl:NamedIndividual rdf:about="http://purl.obolibrary.org/obo/GAZ_00015408">
        <rdf:type rdf:resource="http://purl.obolibrary.org/obo/ENVO_00000004"/>
        <obo:RO_0001025 rdf:resource="http://purl.obolibrary.org/obo/GAZ_00005374"/>
        <obo:IAO_0000115>A district in southwestern Uganda. Rukungiri District is bordered by Bushenyi District to the north and northeast, Ntungamo District to the southeast, Kabale District to the south, Kanungu District to the west and the Democratic Republic of the Congo to the northwest.</obo:IAO_0000115>
        <oboInOwl:hasOBONamespace>GAZ</oboInOwl:hasOBONamespace>
        <oboInOwl:id>GAZ:00015408</oboInOwl:id>
        <rdfs:label>Rukungiri District</rdfs:label>
    </owl:NamedIndividual>
    


    <!-- http://purl.obolibrary.org/obo/GAZ_00015409 -->

    <owl:NamedIndividual rdf:about="http://purl.obolibrary.org/obo/GAZ_00015409">
        <rdf:type rdf:resource="http://purl.obolibrary.org/obo/ENVO_00000004"/>
        <obo:RO_0001025 rdf:resource="http://purl.obolibrary.org/obo/GAZ_00005374"/>
        <obo:IAO_0000115>A district in southwestern Uganda. Ntungamo District is bordered by Rwanda to the south, Isingiro District to the east, Mbarara District to the northeast, Bushenyi District to the north, Rukungiri District to the northwest and Kabale District to the southwest.</obo:IAO_0000115>
        <oboInOwl:hasOBONamespace>GAZ</oboInOwl:hasOBONamespace>
        <oboInOwl:id>GAZ:00015409</oboInOwl:id>
        <rdfs:label>Ntungamo District</rdfs:label>
    </owl:NamedIndividual>
    


    <!-- http://purl.obolibrary.org/obo/GAZ_00015410 -->

    <owl:NamedIndividual rdf:about="http://purl.obolibrary.org/obo/GAZ_00015410">
        <rdf:type rdf:resource="http://purl.obolibrary.org/obo/ENVO_00000004"/>
        <obo:RO_0001025 rdf:resource="http://purl.obolibrary.org/obo/GAZ_00005374"/>
        <obo:IAO_0000115>A district in southwestern Uganda. Kisoro District is bordered by Kanungu District to the north, Kabale District to the east, the Republic of Rwanda to the south and the Democratic Republic of the Congo to the west.</obo:IAO_0000115>
        <oboInOwl:hasOBONamespace>GAZ</oboInOwl:hasOBONamespace>
        <oboInOwl:id>GAZ:00015410</oboInOwl:id>
        <rdfs:label>Kisoro District</rdfs:label>
    </owl:NamedIndividual>
    


    <!-- http://purl.obolibrary.org/obo/GAZ_00015412 -->

    <owl:NamedIndividual rdf:about="http://purl.obolibrary.org/obo/GAZ_00015412">
        <obo:RO_0001025 rdf:resource="http://purl.obolibrary.org/obo/GAZ_00015338"/>
        <obo:IAO_0000115>A county (third-level administrative division) of Uganda.</obo:IAO_0000115>
        <oboInOwl:hasOBONamespace>GAZ</oboInOwl:hasOBONamespace>
        <oboInOwl:id>GAZ:00015412</oboInOwl:id>
        <rdfs:label>Kyadondo County</rdfs:label>
    </owl:NamedIndividual>
    


    <!-- http://purl.obolibrary.org/obo/GAZ_00015413 -->

    <owl:NamedIndividual rdf:about="http://purl.obolibrary.org/obo/GAZ_00015413">
        <obo:RO_0001025 rdf:resource="http://purl.obolibrary.org/obo/GAZ_00015338"/>
    </owl:NamedIndividual>
    


    <!-- http://purl.obolibrary.org/obo/GAZ_00015414 -->

    <owl:NamedIndividual rdf:about="http://purl.obolibrary.org/obo/GAZ_00015414">
        <obo:RO_0001025 rdf:resource="http://purl.obolibrary.org/obo/GAZ_00015338"/>
        <obo:IAO_0000115>A county (third-level administrative division) of Uganda.</obo:IAO_0000115>
        <oboInOwl:hasOBONamespace>GAZ</oboInOwl:hasOBONamespace>
        <oboInOwl:id>GAZ:00015414</oboInOwl:id>
        <rdfs:label>Busiro County</rdfs:label>
    </owl:NamedIndividual>
    


    <!-- http://purl.obolibrary.org/obo/GAZ_00015415 -->

    <owl:NamedIndividual rdf:about="http://purl.obolibrary.org/obo/GAZ_00015415">
        <obo:RO_0001025 rdf:resource="http://purl.obolibrary.org/obo/GAZ_00015371"/>
        <obo:IAO_0000115>A county (third-level administrative division) of Uganda.</obo:IAO_0000115>
        <oboInOwl:hasOBONamespace>GAZ</oboInOwl:hasOBONamespace>
        <oboInOwl:id>GAZ:00015415</oboInOwl:id>
        <rdfs:label>Tororo County</rdfs:label>
    </owl:NamedIndividual>
    


    <!-- http://purl.obolibrary.org/obo/GAZ_00015416 -->

    <owl:NamedIndividual rdf:about="http://purl.obolibrary.org/obo/GAZ_00015416">
        <obo:RO_0001025 rdf:resource="http://purl.obolibrary.org/obo/GAZ_00015371"/>
        <obo:IAO_0000115>A county (third-level administrative division) of Uganda.</obo:IAO_0000115>
        <oboInOwl:hasOBONamespace>GAZ</oboInOwl:hasOBONamespace>
        <oboInOwl:id>GAZ:00015416</oboInOwl:id>
        <rdfs:label>Kisoko County</rdfs:label>
    </owl:NamedIndividual>
    


    <!-- http://purl.obolibrary.org/obo/GAZ_00015417 -->

    <owl:NamedIndividual rdf:about="http://purl.obolibrary.org/obo/GAZ_00015417">
        <obo:RO_0001025 rdf:resource="http://purl.obolibrary.org/obo/GAZ_00015372"/>
        <obo:IAO_0000115>A county (third-level administrative division) of Uganda.</obo:IAO_0000115>
        <oboInOwl:hasOBONamespace>GAZ</oboInOwl:hasOBONamespace>
        <oboInOwl:id>GAZ:00015417</oboInOwl:id>
        <rdfs:label>Serere County</rdfs:label>
    </owl:NamedIndividual>
    


    <!-- http://purl.obolibrary.org/obo/GAZ_00015418 -->

    <owl:NamedIndividual rdf:about="http://purl.obolibrary.org/obo/GAZ_00015418">
        <obo:RO_0001025 rdf:resource="http://purl.obolibrary.org/obo/GAZ_00015372"/>
        <obo:IAO_0000115>A county (third-level administrative division) of Uganda.</obo:IAO_0000115>
        <oboInOwl:hasOBONamespace>GAZ</oboInOwl:hasOBONamespace>
        <oboInOwl:id>GAZ:00015418</oboInOwl:id>
        <rdfs:label>Soroti County</rdfs:label>
    </owl:NamedIndividual>
    


    <!-- http://purl.obolibrary.org/obo/GAZ_00015419 -->

    <owl:NamedIndividual rdf:about="http://purl.obolibrary.org/obo/GAZ_00015419">
        <obo:RO_0001025 rdf:resource="http://purl.obolibrary.org/obo/GAZ_00015372"/>
        <obo:IAO_0000115>A county (third-level administrative division) of Uganda.</obo:IAO_0000115>
        <oboInOwl:hasOBONamespace>GAZ</oboInOwl:hasOBONamespace>
        <oboInOwl:id>GAZ:00015419</oboInOwl:id>
        <rdfs:label>Kasilo County</rdfs:label>
    </owl:NamedIndividual>
    


    <!-- http://purl.obolibrary.org/obo/GAZ_00015420 -->

    <owl:NamedIndividual rdf:about="http://purl.obolibrary.org/obo/GAZ_00015420">
        <obo:RO_0001025 rdf:resource="http://purl.obolibrary.org/obo/GAZ_00015369"/>
        <obo:IAO_0000115>A county (third-level administrative division) of Uganda.</obo:IAO_0000115>
        <oboInOwl:hasOBONamespace>GAZ</oboInOwl:hasOBONamespace>
        <oboInOwl:id>GAZ:00015420</oboInOwl:id>
        <rdfs:label>Bulambuli County</rdfs:label>
    </owl:NamedIndividual>
    


    <!-- http://purl.obolibrary.org/obo/GAZ_00015421 -->

    <owl:NamedIndividual rdf:about="http://purl.obolibrary.org/obo/GAZ_00015421">
        <obo:RO_0001025 rdf:resource="http://purl.obolibrary.org/obo/GAZ_00015369"/>
        <obo:IAO_0000115>A county (third-level administrative division) of Uganda.</obo:IAO_0000115>
        <oboInOwl:hasOBONamespace>GAZ</oboInOwl:hasOBONamespace>
        <oboInOwl:id>GAZ:00015421</oboInOwl:id>
        <rdfs:label>Budadiri County</rdfs:label>
    </owl:NamedIndividual>
    


    <!-- http://purl.obolibrary.org/obo/GAZ_00015422 -->

    <owl:NamedIndividual rdf:about="http://purl.obolibrary.org/obo/GAZ_00015422">
        <obo:RO_0001025 rdf:resource="http://purl.obolibrary.org/obo/GAZ_00015349"/>
        <obo:IAO_0000115>A county (third-level administrative division) of Uganda.</obo:IAO_0000115>
        <oboInOwl:hasOBONamespace>GAZ</oboInOwl:hasOBONamespace>
        <oboInOwl:id>GAZ:00015422</oboInOwl:id>
        <rdfs:label>Lwemiyaga County</rdfs:label>
    </owl:NamedIndividual>
    


    <!-- http://purl.obolibrary.org/obo/GAZ_00015423 -->

    <owl:NamedIndividual rdf:about="http://purl.obolibrary.org/obo/GAZ_00015423">
        <obo:RO_0001025 rdf:resource="http://purl.obolibrary.org/obo/GAZ_00015349"/>
        <obo:IAO_0000115>A county (third-level administrative division) of Uganda.</obo:IAO_0000115>
        <oboInOwl:hasOBONamespace>GAZ</oboInOwl:hasOBONamespace>
        <oboInOwl:id>GAZ:00015423</oboInOwl:id>
        <rdfs:label>Mawogola County</rdfs:label>
    </owl:NamedIndividual>
    


    <!-- http://purl.obolibrary.org/obo/GAZ_00015424 -->

    <owl:NamedIndividual rdf:about="http://purl.obolibrary.org/obo/GAZ_00015424">
        <obo:RO_0001025 rdf:resource="http://purl.obolibrary.org/obo/GAZ_00015345"/>
        <obo:IAO_0000115>A county (third-level administrative division) of Uganda.</obo:IAO_0000115>
        <oboInOwl:hasOBONamespace>GAZ</oboInOwl:hasOBONamespace>
        <oboInOwl:id>GAZ:00015424</oboInOwl:id>
        <rdfs:label>Kakuuto County</rdfs:label>
    </owl:NamedIndividual>
    


    <!-- http://purl.obolibrary.org/obo/GAZ_00015425 -->

    <owl:NamedIndividual rdf:about="http://purl.obolibrary.org/obo/GAZ_00015425">
        <obo:RO_0001025 rdf:resource="http://purl.obolibrary.org/obo/GAZ_00015345"/>
        <obo:IAO_0000115>A county (third-level administrative division) of Uganda.</obo:IAO_0000115>
        <oboInOwl:hasOBONamespace>GAZ</oboInOwl:hasOBONamespace>
        <oboInOwl:id>GAZ:00015425</oboInOwl:id>
        <rdfs:label>Kooki County</rdfs:label>
    </owl:NamedIndividual>
    


    <!-- http://purl.obolibrary.org/obo/GAZ_00015426 -->

    <owl:NamedIndividual rdf:about="http://purl.obolibrary.org/obo/GAZ_00015426">
        <obo:RO_0001025 rdf:resource="http://purl.obolibrary.org/obo/GAZ_00015345"/>
        <obo:IAO_0000115>A county (third-level administrative division) of Uganda.</obo:IAO_0000115>
        <oboInOwl:hasOBONamespace>GAZ</oboInOwl:hasOBONamespace>
        <oboInOwl:id>GAZ:00015426</oboInOwl:id>
        <rdfs:label>Kyotera County</rdfs:label>
    </owl:NamedIndividual>
    


    <!-- http://purl.obolibrary.org/obo/GAZ_00015427 -->

    <owl:NamedIndividual rdf:about="http://purl.obolibrary.org/obo/GAZ_00015427">
        <obo:RO_0001025 rdf:resource="http://purl.obolibrary.org/obo/GAZ_00015345"/>
        <obo:IAO_0000115>A county (third-level administrative division) of Uganda.</obo:IAO_0000115>
        <oboInOwl:hasOBONamespace>GAZ</oboInOwl:hasOBONamespace>
        <oboInOwl:id>GAZ:00015427</oboInOwl:id>
        <rdfs:label>Kabula County</rdfs:label>
    </owl:NamedIndividual>
    


    <!-- http://purl.obolibrary.org/obo/GAZ_00015428 -->

    <owl:NamedIndividual rdf:about="http://purl.obolibrary.org/obo/GAZ_00015428">
        <obo:RO_0001025 rdf:resource="http://purl.obolibrary.org/obo/GAZ_00015348"/>
        <obo:IAO_0000115>A county (third-level administrative division) of Uganda.</obo:IAO_0000115>
        <oboInOwl:hasOBONamespace>GAZ</oboInOwl:hasOBONamespace>
        <oboInOwl:id>GAZ:00015428</oboInOwl:id>
        <rdfs:label>Buruli County</rdfs:label>
    </owl:NamedIndividual>
    


    <!-- http://purl.obolibrary.org/obo/GAZ_00015430 -->

    <owl:NamedIndividual rdf:about="http://purl.obolibrary.org/obo/GAZ_00015430">
        <obo:RO_0001025 rdf:resource="http://purl.obolibrary.org/obo/GAZ_00015342"/>
        <obo:IAO_0000115>A county (third-level administrative division) of Uganda.</obo:IAO_0000115>
        <oboInOwl:hasOBONamespace>GAZ</oboInOwl:hasOBONamespace>
        <oboInOwl:id>GAZ:00015430</oboInOwl:id>
        <rdfs:label>Buvuma Islands County</rdfs:label>
    </owl:NamedIndividual>
    


    <!-- http://purl.obolibrary.org/obo/GAZ_00015431 -->

    <owl:NamedIndividual rdf:about="http://purl.obolibrary.org/obo/GAZ_00015431">
        <obo:RO_0001025 rdf:resource="http://purl.obolibrary.org/obo/GAZ_00015342"/>
        <obo:IAO_0000115>A county (third-level administrative division) of Uganda.</obo:IAO_0000115>
        <oboInOwl:hasOBONamespace>GAZ</oboInOwl:hasOBONamespace>
        <oboInOwl:id>GAZ:00015431</oboInOwl:id>
        <rdfs:label>Mukono County</rdfs:label>
    </owl:NamedIndividual>
    


    <!-- http://purl.obolibrary.org/obo/GAZ_00015432 -->

    <owl:NamedIndividual rdf:about="http://purl.obolibrary.org/obo/GAZ_00015432">
        <obo:RO_0001025 rdf:resource="http://purl.obolibrary.org/obo/GAZ_00015342"/>
        <obo:IAO_0000115>A county (third-level administrative division) of Uganda.</obo:IAO_0000115>
        <oboInOwl:hasOBONamespace>GAZ</oboInOwl:hasOBONamespace>
        <oboInOwl:id>GAZ:00015432</oboInOwl:id>
        <rdfs:label>Nakifuma County</rdfs:label>
    </owl:NamedIndividual>
    


    <!-- http://purl.obolibrary.org/obo/GAZ_00015433 -->

    <owl:NamedIndividual rdf:about="http://purl.obolibrary.org/obo/GAZ_00015433">
        <obo:RO_0001025 rdf:resource="http://purl.obolibrary.org/obo/GAZ_00015342"/>
        <obo:IAO_0000115>A county (third-level administrative division) of Uganda.</obo:IAO_0000115>
        <oboInOwl:hasOBONamespace>GAZ</oboInOwl:hasOBONamespace>
        <oboInOwl:id>GAZ:00015433</oboInOwl:id>
        <rdfs:label>Buyikwe County</rdfs:label>
    </owl:NamedIndividual>
    


    <!-- http://purl.obolibrary.org/obo/GAZ_00015434 -->

    <owl:NamedIndividual rdf:about="http://purl.obolibrary.org/obo/GAZ_00015434">
        <obo:RO_0001025 rdf:resource="http://purl.obolibrary.org/obo/GAZ_00015339"/>
        <obo:IAO_0000115>A county (third-level administrative division) of Uganda.</obo:IAO_0000115>
        <oboInOwl:hasOBONamespace>GAZ</oboInOwl:hasOBONamespace>
        <oboInOwl:id>GAZ:00015434</oboInOwl:id>
        <rdfs:label>Buwekula County</rdfs:label>
    </owl:NamedIndividual>
    


    <!-- http://purl.obolibrary.org/obo/GAZ_00015435 -->

    <owl:NamedIndividual rdf:about="http://purl.obolibrary.org/obo/GAZ_00015435">
        <obo:RO_0001025 rdf:resource="http://purl.obolibrary.org/obo/GAZ_00015339"/>
        <obo:IAO_0000115>A county (third-level administrative division) of Uganda.</obo:IAO_0000115>
        <oboInOwl:hasOBONamespace>GAZ</oboInOwl:hasOBONamespace>
        <oboInOwl:id>GAZ:00015435</oboInOwl:id>
        <rdfs:label>Kassanda County</rdfs:label>
    </owl:NamedIndividual>
    


    <!-- http://purl.obolibrary.org/obo/GAZ_00015436 -->

    <owl:NamedIndividual rdf:about="http://purl.obolibrary.org/obo/GAZ_00015436">
        <obo:RO_0001025 rdf:resource="http://purl.obolibrary.org/obo/GAZ_00005378"/>
        <obo:IAO_0000115>A county (third-level administrative division) of Uganda.</obo:IAO_0000115>
        <oboInOwl:hasOBONamespace>GAZ</oboInOwl:hasOBONamespace>
        <oboInOwl:id>GAZ:00015436</oboInOwl:id>
        <rdfs:label>Butambala County</rdfs:label>
    </owl:NamedIndividual>
    


    <!-- http://purl.obolibrary.org/obo/GAZ_00015437 -->

    <owl:NamedIndividual rdf:about="http://purl.obolibrary.org/obo/GAZ_00015437">
        <obo:RO_0001025 rdf:resource="http://purl.obolibrary.org/obo/GAZ_00005378"/>
        <obo:IAO_0000115>A county (third-level administrative division) of Uganda.</obo:IAO_0000115>
        <oboInOwl:hasOBONamespace>GAZ</oboInOwl:hasOBONamespace>
        <oboInOwl:id>GAZ:00015437</oboInOwl:id>
        <rdfs:label>Mawokota County</rdfs:label>
    </owl:NamedIndividual>
    


    <!-- http://purl.obolibrary.org/obo/GAZ_00015438 -->

    <owl:NamedIndividual rdf:about="http://purl.obolibrary.org/obo/GAZ_00015438">
        <obo:RO_0001025 rdf:resource="http://purl.obolibrary.org/obo/GAZ_00005378"/>
        <obo:IAO_0000115>A county (third-level administrative division) of Uganda.</obo:IAO_0000115>
        <oboInOwl:hasOBONamespace>GAZ</oboInOwl:hasOBONamespace>
        <oboInOwl:id>GAZ:00015438</oboInOwl:id>
        <rdfs:label>Gomba County</rdfs:label>
    </owl:NamedIndividual>
    


    <!-- http://purl.obolibrary.org/obo/GAZ_00015439 -->

    <owl:NamedIndividual rdf:about="http://purl.obolibrary.org/obo/GAZ_00015439">
        <obo:RO_0001025 rdf:resource="http://purl.obolibrary.org/obo/GAZ_00015344"/>
        <obo:IAO_0000115>A county (third-level administrative division) of Uganda.</obo:IAO_0000115>
        <oboInOwl:hasOBONamespace>GAZ</oboInOwl:hasOBONamespace>
        <oboInOwl:id>GAZ:00015439</oboInOwl:id>
        <rdfs:label>Bujumba County</rdfs:label>
    </owl:NamedIndividual>
    


    <!-- http://purl.obolibrary.org/obo/GAZ_00015440 -->

    <owl:NamedIndividual rdf:about="http://purl.obolibrary.org/obo/GAZ_00015440">
        <obo:RO_0001025 rdf:resource="http://purl.obolibrary.org/obo/GAZ_00015344"/>
        <obo:IAO_0000115>A county (third-level administrative division) of Uganda.</obo:IAO_0000115>
        <oboInOwl:hasOBONamespace>GAZ</oboInOwl:hasOBONamespace>
        <oboInOwl:id>GAZ:00015440</oboInOwl:id>
        <rdfs:label>Kyamuswa County</rdfs:label>
    </owl:NamedIndividual>
    


    <!-- http://purl.obolibrary.org/obo/GAZ_00015442 -->

    <owl:NamedIndividual rdf:about="http://purl.obolibrary.org/obo/GAZ_00015442">
        <obo:RO_0001025 rdf:resource="http://purl.obolibrary.org/obo/GAZ_00015341"/>
        <obo:IAO_0000115>A county (third-level administrative division) of Uganda.</obo:IAO_0000115>
        <oboInOwl:hasOBONamespace>GAZ</oboInOwl:hasOBONamespace>
        <oboInOwl:id>GAZ:00015442</oboInOwl:id>
        <rdfs:label>Bbaale County</rdfs:label>
    </owl:NamedIndividual>
    


    <!-- http://purl.obolibrary.org/obo/GAZ_00015443 -->

    <owl:NamedIndividual rdf:about="http://purl.obolibrary.org/obo/GAZ_00015443">
        <obo:RO_0001025 rdf:resource="http://purl.obolibrary.org/obo/GAZ_00015341"/>
        <obo:IAO_0000115>A county (third-level administrative division) of Uganda.</obo:IAO_0000115>
        <oboInOwl:hasOBONamespace>GAZ</oboInOwl:hasOBONamespace>
        <oboInOwl:id>GAZ:00015443</oboInOwl:id>
        <rdfs:label>Ntenjeru County</rdfs:label>
    </owl:NamedIndividual>
    


    <!-- http://purl.obolibrary.org/obo/GAZ_00015445 -->

    <owl:NamedIndividual rdf:about="http://purl.obolibrary.org/obo/GAZ_00015445">
        <obo:RO_0001025 rdf:resource="http://purl.obolibrary.org/obo/GAZ_00015340"/>
        <obo:IAO_0000115>A county (third-level administrative division) of Uganda.</obo:IAO_0000115>
        <oboInOwl:hasOBONamespace>GAZ</oboInOwl:hasOBONamespace>
        <oboInOwl:id>GAZ:00015445</oboInOwl:id>
        <rdfs:label>Katikamu County</rdfs:label>
    </owl:NamedIndividual>
    


    <!-- http://purl.obolibrary.org/obo/GAZ_00015447 -->

    <owl:NamedIndividual rdf:about="http://purl.obolibrary.org/obo/GAZ_00015447">
        <obo:RO_0001025 rdf:resource="http://purl.obolibrary.org/obo/GAZ_00005380"/>
        <obo:IAO_0000115>A county (third-level administrative division) of Uganda.</obo:IAO_0000115>
        <oboInOwl:hasOBONamespace>GAZ</oboInOwl:hasOBONamespace>
        <oboInOwl:id>GAZ:00015447</oboInOwl:id>
        <rdfs:label>Bukomansimbi County</rdfs:label>
    </owl:NamedIndividual>
    


    <!-- http://purl.obolibrary.org/obo/GAZ_00015448 -->

    <owl:NamedIndividual rdf:about="http://purl.obolibrary.org/obo/GAZ_00015448">
        <obo:RO_0001025 rdf:resource="http://purl.obolibrary.org/obo/GAZ_00005380"/>
        <obo:IAO_0000115>A county (third-level administrative division) of Uganda.</obo:IAO_0000115>
        <oboInOwl:hasOBONamespace>GAZ</oboInOwl:hasOBONamespace>
        <oboInOwl:id>GAZ:00015448</oboInOwl:id>
        <rdfs:label>Kalungu County</rdfs:label>
    </owl:NamedIndividual>
    


    <!-- http://purl.obolibrary.org/obo/GAZ_00015449 -->

    <owl:NamedIndividual rdf:about="http://purl.obolibrary.org/obo/GAZ_00015449">
        <obo:RO_0001025 rdf:resource="http://purl.obolibrary.org/obo/GAZ_00005380"/>
        <obo:IAO_0000115>A county (third-level administrative division) of Uganda.</obo:IAO_0000115>
        <oboInOwl:hasOBONamespace>GAZ</oboInOwl:hasOBONamespace>
        <oboInOwl:id>GAZ:00015449</oboInOwl:id>
        <rdfs:label>Bukoto County</rdfs:label>
    </owl:NamedIndividual>
    


    <!-- http://purl.obolibrary.org/obo/GAZ_00015450 -->

    <owl:NamedIndividual rdf:about="http://purl.obolibrary.org/obo/GAZ_00015450">
        <obo:RO_0001025 rdf:resource="http://purl.obolibrary.org/obo/GAZ_00015347"/>
        <obo:IAO_0000115>A county (third-level administrative division) of Uganda.</obo:IAO_0000115>
        <oboInOwl:hasOBONamespace>GAZ</oboInOwl:hasOBONamespace>
        <oboInOwl:id>GAZ:00015450</oboInOwl:id>
        <rdfs:label>Busujju County</rdfs:label>
    </owl:NamedIndividual>
    


    <!-- http://purl.obolibrary.org/obo/GAZ_00015451 -->

    <owl:NamedIndividual rdf:about="http://purl.obolibrary.org/obo/GAZ_00015451">
        <obo:RO_0001025 rdf:resource="http://purl.obolibrary.org/obo/GAZ_00015347"/>
        <obo:IAO_0000115>A county (third-level administrative division) of Uganda.</obo:IAO_0000115>
        <oboInOwl:hasOBONamespace>GAZ</oboInOwl:hasOBONamespace>
        <oboInOwl:id>GAZ:00015451</oboInOwl:id>
        <rdfs:label>Mityana County</rdfs:label>
    </owl:NamedIndividual>
    


    <!-- http://purl.obolibrary.org/obo/GAZ_00015452 -->

    <owl:NamedIndividual rdf:about="http://purl.obolibrary.org/obo/GAZ_00015452">
        <obo:RO_0001025 rdf:resource="http://purl.obolibrary.org/obo/GAZ_00000007"/>
        <obo:RO_0001025 rdf:resource="http://purl.obolibrary.org/obo/GAZ_00005380"/>
        <obo:IAO_0000115>A very large monictic freshwater lake bordering Kenya, Tanzania and Uganda.</obo:IAO_0000115>
        <oboInOwl:hasOBONamespace>GAZ</oboInOwl:hasOBONamespace>
        <oboInOwl:id>GAZ:00015452</oboInOwl:id>
        <rdfs:label>Lake Victoria</rdfs:label>
    </owl:NamedIndividual>
    


    <!-- http://purl.obolibrary.org/obo/GAZ_00015453 -->

    <owl:NamedIndividual rdf:about="http://purl.obolibrary.org/obo/GAZ_00015453">
        <obo:RO_0001025 rdf:resource="http://purl.obolibrary.org/obo/GAZ_00015430"/>
        <obo:RO_0001025 rdf:resource="http://purl.obolibrary.org/obo/GAZ_00124567"/>
        <obo:IAO_0000115>A chain of more than fifty smaller islands, a few km off the northern shore of Lake Victoria, Uganda in the Napoleon Gulf.</obo:IAO_0000115>
        <oboInOwl:hasOBONamespace>GAZ</oboInOwl:hasOBONamespace>
        <oboInOwl:id>GAZ:00015453</oboInOwl:id>
        <rdfs:label>Buvuma Islands</rdfs:label>
    </owl:NamedIndividual>
    


    <!-- http://purl.obolibrary.org/obo/GAZ_00015454 -->

    <owl:NamedIndividual rdf:about="http://purl.obolibrary.org/obo/GAZ_00015454">
        <obo:RO_0001025 rdf:resource="http://purl.obolibrary.org/obo/GAZ_00015353"/>
        <obo:IAO_0000115>A county (third-level administrative division) of Uganda.</obo:IAO_0000115>
        <oboInOwl:hasOBONamespace>GAZ</oboInOwl:hasOBONamespace>
        <oboInOwl:id>GAZ:00015454</oboInOwl:id>
        <rdfs:label>Amuria County</rdfs:label>
    </owl:NamedIndividual>
    


    <!-- http://purl.obolibrary.org/obo/GAZ_00015455 -->

    <owl:NamedIndividual rdf:about="http://purl.obolibrary.org/obo/GAZ_00015455">
        <obo:RO_0001025 rdf:resource="http://purl.obolibrary.org/obo/GAZ_00015353"/>
        <obo:IAO_0000115>A county (third-level administrative division) of Uganda.</obo:IAO_0000115>
        <oboInOwl:hasOBONamespace>GAZ</oboInOwl:hasOBONamespace>
        <oboInOwl:id>GAZ:00015455</oboInOwl:id>
        <rdfs:label>Kapelebyong County</rdfs:label>
    </owl:NamedIndividual>
    


    <!-- http://purl.obolibrary.org/obo/GAZ_00015456 -->

    <owl:NamedIndividual rdf:about="http://purl.obolibrary.org/obo/GAZ_00015456">
        <obo:RO_0001025 rdf:resource="http://purl.obolibrary.org/obo/GAZ_00015365"/>
        <obo:IAO_0000115>A county (third-level administrative division) of Uganda.</obo:IAO_0000115>
        <oboInOwl:hasOBONamespace>GAZ</oboInOwl:hasOBONamespace>
        <oboInOwl:id>GAZ:00015456</oboInOwl:id>
        <rdfs:label>Budaka County</rdfs:label>
    </owl:NamedIndividual>
    


    <!-- http://purl.obolibrary.org/obo/GAZ_00015457 -->

    <owl:NamedIndividual rdf:about="http://purl.obolibrary.org/obo/GAZ_00015457">
        <obo:RO_0001025 rdf:resource="http://purl.obolibrary.org/obo/GAZ_00015365"/>
        <obo:IAO_0000115>A county (third-level administrative division) of Uganda.</obo:IAO_0000115>
        <oboInOwl:hasOBONamespace>GAZ</oboInOwl:hasOBONamespace>
        <oboInOwl:id>GAZ:00015457</oboInOwl:id>
        <rdfs:label>Butebo County</rdfs:label>
    </owl:NamedIndividual>
    


    <!-- http://purl.obolibrary.org/obo/GAZ_00015462 -->

    <owl:NamedIndividual rdf:about="http://purl.obolibrary.org/obo/GAZ_00015462">
        <obo:RO_0001025 rdf:resource="http://purl.obolibrary.org/obo/GAZ_00015358"/>
        <obo:IAO_0000115>A county (third-level administrative division) of Uganda.</obo:IAO_0000115>
        <oboInOwl:hasOBONamespace>GAZ</oboInOwl:hasOBONamespace>
        <oboInOwl:id>GAZ:00015462</oboInOwl:id>
        <rdfs:label>Bugweri County</rdfs:label>
    </owl:NamedIndividual>
    


    <!-- http://purl.obolibrary.org/obo/GAZ_00015463 -->

    <owl:NamedIndividual rdf:about="http://purl.obolibrary.org/obo/GAZ_00015463">
        <obo:RO_0001025 rdf:resource="http://purl.obolibrary.org/obo/GAZ_00015358"/>
        <obo:IAO_0000115>A county (third-level administrative division) of Uganda.</obo:IAO_0000115>
        <oboInOwl:hasOBONamespace>GAZ</oboInOwl:hasOBONamespace>
        <oboInOwl:id>GAZ:00015463</oboInOwl:id>
        <rdfs:label>Kigulu County</rdfs:label>
    </owl:NamedIndividual>
    


    <!-- http://purl.obolibrary.org/obo/GAZ_00015464 -->

    <owl:NamedIndividual rdf:about="http://purl.obolibrary.org/obo/GAZ_00015464">
        <obo:RO_0001025 rdf:resource="http://purl.obolibrary.org/obo/GAZ_00015358"/>
        <obo:IAO_0000115>A county (third-level administrative division) of Uganda.</obo:IAO_0000115>
        <oboInOwl:hasOBONamespace>GAZ</oboInOwl:hasOBONamespace>
        <oboInOwl:id>GAZ:00015464</oboInOwl:id>
        <rdfs:label>Luuka County</rdfs:label>
    </owl:NamedIndividual>
    


    <!-- http://purl.obolibrary.org/obo/GAZ_00015465 -->

    <owl:NamedIndividual rdf:about="http://purl.obolibrary.org/obo/GAZ_00015465">
        <obo:RO_0001025 rdf:resource="http://purl.obolibrary.org/obo/GAZ_00015351"/>
        <obo:IAO_0000115>A county (third-level administrative division) of Uganda.</obo:IAO_0000115>
        <oboInOwl:hasOBONamespace>GAZ</oboInOwl:hasOBONamespace>
        <oboInOwl:id>GAZ:00015465</oboInOwl:id>
        <rdfs:label>Butembe County</rdfs:label>
    </owl:NamedIndividual>
    


    <!-- http://purl.obolibrary.org/obo/GAZ_00015466 -->

    <owl:NamedIndividual rdf:about="http://purl.obolibrary.org/obo/GAZ_00015466">
        <obo:RO_0001025 rdf:resource="http://purl.obolibrary.org/obo/GAZ_00015351"/>
        <obo:IAO_0000115>A county (third-level administrative division) of Uganda.</obo:IAO_0000115>
        <oboInOwl:hasOBONamespace>GAZ</oboInOwl:hasOBONamespace>
        <oboInOwl:id>GAZ:00015466</oboInOwl:id>
        <rdfs:label>Municipality of Jinja</rdfs:label>
    </owl:NamedIndividual>
    


    <!-- http://purl.obolibrary.org/obo/GAZ_00015467 -->

    <owl:NamedIndividual rdf:about="http://purl.obolibrary.org/obo/GAZ_00015467">
        <obo:RO_0001025 rdf:resource="http://purl.obolibrary.org/obo/GAZ_00015351"/>
        <obo:IAO_0000115>A county (third-level administrative division) of Uganda.</obo:IAO_0000115>
        <oboInOwl:hasOBONamespace>GAZ</oboInOwl:hasOBONamespace>
        <oboInOwl:id>GAZ:00015467</oboInOwl:id>
        <rdfs:label>Kagoma County</rdfs:label>
    </owl:NamedIndividual>
    


    <!-- http://purl.obolibrary.org/obo/GAZ_00015468 -->

    <owl:NamedIndividual rdf:about="http://purl.obolibrary.org/obo/GAZ_00015468">
        <obo:RO_0001025 rdf:resource="http://purl.obolibrary.org/obo/GAZ_00015355"/>
        <obo:IAO_0000115>A county (third-level administrative division) of Uganda.</obo:IAO_0000115>
        <oboInOwl:hasOBONamespace>GAZ</oboInOwl:hasOBONamespace>
        <oboInOwl:id>GAZ:00015468</oboInOwl:id>
        <rdfs:label>Kaberamaido County</rdfs:label>
    </owl:NamedIndividual>
    


    <!-- http://purl.obolibrary.org/obo/GAZ_00015469 -->

    <owl:NamedIndividual rdf:about="http://purl.obolibrary.org/obo/GAZ_00015469">
        <obo:RO_0001025 rdf:resource="http://purl.obolibrary.org/obo/GAZ_00015355"/>
        <obo:IAO_0000115>A county (third-level administrative division) of Uganda.</obo:IAO_0000115>
        <oboInOwl:hasOBONamespace>GAZ</oboInOwl:hasOBONamespace>
        <oboInOwl:id>GAZ:00015469</oboInOwl:id>
        <rdfs:label>Kalaki County</rdfs:label>
    </owl:NamedIndividual>
    


    <!-- http://purl.obolibrary.org/obo/GAZ_00015470 -->

    <owl:NamedIndividual rdf:about="http://purl.obolibrary.org/obo/GAZ_00015470">
        <obo:RO_0001025 rdf:resource="http://purl.obolibrary.org/obo/GAZ_00015360"/>
        <obo:IAO_0000115>A county (third-level administrative division) of Uganda.</obo:IAO_0000115>
        <oboInOwl:hasOBONamespace>GAZ</oboInOwl:hasOBONamespace>
        <oboInOwl:id>GAZ:00015470</oboInOwl:id>
        <rdfs:label>Bulamogi County</rdfs:label>
    </owl:NamedIndividual>
    


    <!-- http://purl.obolibrary.org/obo/GAZ_00015471 -->

    <owl:NamedIndividual rdf:about="http://purl.obolibrary.org/obo/GAZ_00015471">
        <obo:RO_0001025 rdf:resource="http://purl.obolibrary.org/obo/GAZ_00015352"/>
        <obo:IAO_0000115>A county (third-level administrative division) of Uganda.</obo:IAO_0000115>
        <oboInOwl:hasOBONamespace>GAZ</oboInOwl:hasOBONamespace>
        <oboInOwl:id>GAZ:00015471</oboInOwl:id>
        <rdfs:label>Budiope County</rdfs:label>
    </owl:NamedIndividual>
    


    <!-- http://purl.obolibrary.org/obo/GAZ_00015472 -->

    <owl:NamedIndividual rdf:about="http://purl.obolibrary.org/obo/GAZ_00015472">
        <obo:RO_0001025 rdf:resource="http://purl.obolibrary.org/obo/GAZ_00015352"/>
        <obo:IAO_0000115>A county (third-level administrative division) of Uganda.</obo:IAO_0000115>
        <oboInOwl:hasOBONamespace>GAZ</oboInOwl:hasOBONamespace>
        <oboInOwl:id>GAZ:00015472</oboInOwl:id>
        <rdfs:label>Bugabula County</rdfs:label>
    </owl:NamedIndividual>
    


    <!-- http://purl.obolibrary.org/obo/GAZ_00015473 -->

    <owl:NamedIndividual rdf:about="http://purl.obolibrary.org/obo/GAZ_00015473">
        <obo:RO_0001025 rdf:resource="http://purl.obolibrary.org/obo/GAZ_00015352"/>
        <obo:IAO_0000115>A county (third-level administrative division) of Uganda.</obo:IAO_0000115>
        <oboInOwl:hasOBONamespace>GAZ</oboInOwl:hasOBONamespace>
        <oboInOwl:id>GAZ:00015473</oboInOwl:id>
        <rdfs:label>Buzaaya County</rdfs:label>
    </owl:NamedIndividual>
    


    <!-- http://purl.obolibrary.org/obo/GAZ_00015474 -->

    <owl:NamedIndividual rdf:about="http://purl.obolibrary.org/obo/GAZ_00015474">
        <obo:RO_0001025 rdf:resource="http://purl.obolibrary.org/obo/GAZ_00015361"/>
        <obo:IAO_0000115>A county (third-level administrative division) of Uganda.</obo:IAO_0000115>
        <oboInOwl:hasOBONamespace>GAZ</oboInOwl:hasOBONamespace>
        <oboInOwl:id>GAZ:00015474</oboInOwl:id>
        <rdfs:label>Kween County</rdfs:label>
    </owl:NamedIndividual>
    


    <!-- http://purl.obolibrary.org/obo/GAZ_00015475 -->

    <owl:NamedIndividual rdf:about="http://purl.obolibrary.org/obo/GAZ_00015475">
        <obo:RO_0001025 rdf:resource="http://purl.obolibrary.org/obo/GAZ_00015361"/>
        <obo:IAO_0000115>A county (third-level administrative division) of Uganda.</obo:IAO_0000115>
        <oboInOwl:hasOBONamespace>GAZ</oboInOwl:hasOBONamespace>
        <oboInOwl:id>GAZ:00015475</oboInOwl:id>
        <rdfs:label>Tingey County</rdfs:label>
    </owl:NamedIndividual>
    


    <!-- http://purl.obolibrary.org/obo/GAZ_00015477 -->

    <owl:NamedIndividual rdf:about="http://purl.obolibrary.org/obo/GAZ_00015477">
        <obo:RO_0001025 rdf:resource="http://purl.obolibrary.org/obo/GAZ_00015368"/>
        <obo:IAO_0000115>A county (third-level administrative division) of Uganda.</obo:IAO_0000115>
        <oboInOwl:hasOBONamespace>GAZ</oboInOwl:hasOBONamespace>
        <oboInOwl:id>GAZ:00015477</oboInOwl:id>
        <rdfs:label>Kumi County</rdfs:label>
    </owl:NamedIndividual>
    


    <!-- http://purl.obolibrary.org/obo/GAZ_00015478 -->

    <owl:NamedIndividual rdf:about="http://purl.obolibrary.org/obo/GAZ_00015478">
        <obo:RO_0001025 rdf:resource="http://purl.obolibrary.org/obo/GAZ_00015368"/>
        <obo:IAO_0000115>A county (third-level administrative division) of Uganda.</obo:IAO_0000115>
        <oboInOwl:hasOBONamespace>GAZ</oboInOwl:hasOBONamespace>
        <oboInOwl:id>GAZ:00015478</oboInOwl:id>
        <rdfs:label>Ngora County</rdfs:label>
    </owl:NamedIndividual>
    


    <!-- http://purl.obolibrary.org/obo/GAZ_00015479 -->

    <owl:NamedIndividual rdf:about="http://purl.obolibrary.org/obo/GAZ_00015479">
        <obo:RO_0001025 rdf:resource="http://purl.obolibrary.org/obo/GAZ_00015373"/>
        <obo:IAO_0000115>A county (third-level administrative division) of Uganda.</obo:IAO_0000115>
        <oboInOwl:hasOBONamespace>GAZ</oboInOwl:hasOBONamespace>
        <oboInOwl:id>GAZ:00015479</oboInOwl:id>
        <rdfs:label>Bubulo County</rdfs:label>
    </owl:NamedIndividual>
    


    <!-- http://purl.obolibrary.org/obo/GAZ_00015480 -->

    <owl:NamedIndividual rdf:about="http://purl.obolibrary.org/obo/GAZ_00015480">
        <obo:RO_0001025 rdf:resource="http://purl.obolibrary.org/obo/GAZ_00015373"/>
        <obo:IAO_0000115>A county (third-level administrative division) of Uganda.</obo:IAO_0000115>
        <oboInOwl:hasOBONamespace>GAZ</oboInOwl:hasOBONamespace>
        <oboInOwl:id>GAZ:00015480</oboInOwl:id>
        <rdfs:label>Manjiya County</rdfs:label>
    </owl:NamedIndividual>
    


    <!-- http://purl.obolibrary.org/obo/GAZ_00015482 -->

    <owl:NamedIndividual rdf:about="http://purl.obolibrary.org/obo/GAZ_00015482">
        <obo:RO_0001025 rdf:resource="http://purl.obolibrary.org/obo/GAZ_00015367"/>
        <obo:IAO_0000115>A county (third-level administrative division) of Uganda.</obo:IAO_0000115>
        <oboInOwl:hasOBONamespace>GAZ</oboInOwl:hasOBONamespace>
        <oboInOwl:id>GAZ:00015482</oboInOwl:id>
        <rdfs:label>Bungokho County</rdfs:label>
    </owl:NamedIndividual>
    


    <!-- http://purl.obolibrary.org/obo/GAZ_00015483 -->

    <owl:NamedIndividual rdf:about="http://purl.obolibrary.org/obo/GAZ_00015483">
        <obo:RO_0001025 rdf:resource="http://purl.obolibrary.org/obo/GAZ_00015367"/>
        <obo:IAO_0000115>A county (third-level administrative division) of Uganda.</obo:IAO_0000115>
        <oboInOwl:hasOBONamespace>GAZ</oboInOwl:hasOBONamespace>
        <oboInOwl:id>GAZ:00015483</oboInOwl:id>
        <rdfs:label>Municipality of Mbale</rdfs:label>
    </owl:NamedIndividual>
    


    <!-- http://purl.obolibrary.org/obo/GAZ_00015485 -->

    <owl:NamedIndividual rdf:about="http://purl.obolibrary.org/obo/GAZ_00015485">
        <obo:RO_0001025 rdf:resource="http://purl.obolibrary.org/obo/GAZ_00015390"/>
        <obo:IAO_0000115>A county (third-level administrative division) of Uganda.</obo:IAO_0000115>
        <oboInOwl:hasOBONamespace>GAZ</oboInOwl:hasOBONamespace>
        <oboInOwl:id>GAZ:00015485</oboInOwl:id>
        <rdfs:label>East Moyo County</rdfs:label>
    </owl:NamedIndividual>
    


    <!-- http://purl.obolibrary.org/obo/GAZ_00015486 -->

    <owl:NamedIndividual rdf:about="http://purl.obolibrary.org/obo/GAZ_00015486">
        <obo:RO_0001025 rdf:resource="http://purl.obolibrary.org/obo/GAZ_00015388"/>
        <obo:IAO_0000115>A county (third-level administrative division) of Uganda.</obo:IAO_0000115>
        <oboInOwl:hasOBONamespace>GAZ</oboInOwl:hasOBONamespace>
        <oboInOwl:id>GAZ:00015486</oboInOwl:id>
        <rdfs:label>Kyoga County</rdfs:label>
    </owl:NamedIndividual>
    


    <!-- http://purl.obolibrary.org/obo/GAZ_00015487 -->

    <owl:NamedIndividual rdf:about="http://purl.obolibrary.org/obo/GAZ_00015487">
        <obo:RO_0001025 rdf:resource="http://purl.obolibrary.org/obo/GAZ_00015391"/>
        <obo:IAO_0000115>A county (third-level administrative division) of Uganda.</obo:IAO_0000115>
        <oboInOwl:hasOBONamespace>GAZ</oboInOwl:hasOBONamespace>
        <oboInOwl:id>GAZ:00015487</oboInOwl:id>
        <rdfs:label>Kilak County</rdfs:label>
    </owl:NamedIndividual>
    


    <!-- http://purl.obolibrary.org/obo/GAZ_00015488 -->

    <owl:NamedIndividual rdf:about="http://purl.obolibrary.org/obo/GAZ_00015488">
        <obo:RO_0001025 rdf:resource="http://purl.obolibrary.org/obo/GAZ_00015391"/>
        <obo:IAO_0000115>A county (third-level administrative division) of Uganda.</obo:IAO_0000115>
        <oboInOwl:hasOBONamespace>GAZ</oboInOwl:hasOBONamespace>
        <oboInOwl:id>GAZ:00015488</oboInOwl:id>
        <rdfs:label>Nwoya County</rdfs:label>
    </owl:NamedIndividual>
    


    <!-- http://purl.obolibrary.org/obo/GAZ_00015489 -->

    <owl:NamedIndividual rdf:about="http://purl.obolibrary.org/obo/GAZ_00015489">
        <obo:RO_0001025 rdf:resource="http://purl.obolibrary.org/obo/GAZ_00015393"/>
        <obo:IAO_0000115>A county (third-level administrative division) of Uganda.</obo:IAO_0000115>
        <oboInOwl:hasOBONamespace>GAZ</oboInOwl:hasOBONamespace>
        <oboInOwl:id>GAZ:00015489</oboInOwl:id>
        <rdfs:label>Kole County</rdfs:label>
    </owl:NamedIndividual>
    


    <!-- http://purl.obolibrary.org/obo/GAZ_00015490 -->

    <owl:NamedIndividual rdf:about="http://purl.obolibrary.org/obo/GAZ_00015490">
        <obo:RO_0001025 rdf:resource="http://purl.obolibrary.org/obo/GAZ_00015393"/>
        <obo:IAO_0000115>A county (third-level administrative division) of Uganda.</obo:IAO_0000115>
        <oboInOwl:hasOBONamespace>GAZ</oboInOwl:hasOBONamespace>
        <oboInOwl:id>GAZ:00015490</oboInOwl:id>
        <rdfs:label>Kwania County</rdfs:label>
    </owl:NamedIndividual>
    


    <!-- http://purl.obolibrary.org/obo/GAZ_00015491 -->

    <owl:NamedIndividual rdf:about="http://purl.obolibrary.org/obo/GAZ_00015491">
        <obo:RO_0001025 rdf:resource="http://purl.obolibrary.org/obo/GAZ_00015393"/>
        <obo:IAO_0000115>A county (third-level administrative division) of Uganda.</obo:IAO_0000115>
        <oboInOwl:hasOBONamespace>GAZ</oboInOwl:hasOBONamespace>
        <oboInOwl:id>GAZ:00015491</oboInOwl:id>
        <rdfs:label>Maruzi County</rdfs:label>
    </owl:NamedIndividual>
    


    <!-- http://purl.obolibrary.org/obo/GAZ_00015492 -->

    <owl:NamedIndividual rdf:about="http://purl.obolibrary.org/obo/GAZ_00015492">
        <obo:RO_0001025 rdf:resource="http://purl.obolibrary.org/obo/GAZ_00015389"/>
        <obo:IAO_0000115>A county (third-level administrative division) of Uganda.</obo:IAO_0000115>
        <oboInOwl:hasOBONamespace>GAZ</oboInOwl:hasOBONamespace>
        <oboInOwl:id>GAZ:00015492</oboInOwl:id>
        <rdfs:label>Madi-Okollo County</rdfs:label>
    </owl:NamedIndividual>
    


    <!-- http://purl.obolibrary.org/obo/GAZ_00015493 -->

    <owl:NamedIndividual rdf:about="http://purl.obolibrary.org/obo/GAZ_00015493">
        <obo:RO_0001025 rdf:resource="http://purl.obolibrary.org/obo/GAZ_00015389"/>
        <obo:IAO_0000115>A county (third-level administrative division) of Uganda.</obo:IAO_0000115>
        <oboInOwl:hasOBONamespace>GAZ</oboInOwl:hasOBONamespace>
        <oboInOwl:id>GAZ:00015493</oboInOwl:id>
        <rdfs:label>Municipality of Arua</rdfs:label>
    </owl:NamedIndividual>
    


    <!-- http://purl.obolibrary.org/obo/GAZ_00015494 -->

    <owl:NamedIndividual rdf:about="http://purl.obolibrary.org/obo/GAZ_00015494">
        <obo:RO_0001025 rdf:resource="http://purl.obolibrary.org/obo/GAZ_00015389"/>
        <obo:IAO_0000115>A county (third-level administrative division) of Uganda.</obo:IAO_0000115>
        <oboInOwl:hasOBONamespace>GAZ</oboInOwl:hasOBONamespace>
        <oboInOwl:id>GAZ:00015494</oboInOwl:id>
        <rdfs:label>Vurra County</rdfs:label>
    </owl:NamedIndividual>
    


    <!-- http://purl.obolibrary.org/obo/GAZ_00015495 -->

    <owl:NamedIndividual rdf:about="http://purl.obolibrary.org/obo/GAZ_00015495">
        <obo:RO_0001025 rdf:resource="http://purl.obolibrary.org/obo/GAZ_00015389"/>
        <obo:IAO_0000115>A county (third-level administrative division) of Uganda.</obo:IAO_0000115>
        <oboInOwl:hasOBONamespace>GAZ</oboInOwl:hasOBONamespace>
        <oboInOwl:id>GAZ:00015495</oboInOwl:id>
        <rdfs:label>Ayivu County</rdfs:label>
    </owl:NamedIndividual>
    


    <!-- http://purl.obolibrary.org/obo/GAZ_00015497 -->

    <owl:NamedIndividual rdf:about="http://purl.obolibrary.org/obo/GAZ_00015497">
        <obo:RO_0001025 rdf:resource="http://purl.obolibrary.org/obo/GAZ_00009913"/>
        <obo:IAO_0000115>A county (third-level administrative division) of Uganda.</obo:IAO_0000115>
        <oboInOwl:hasOBONamespace>GAZ</oboInOwl:hasOBONamespace>
        <oboInOwl:id>GAZ:00015497</oboInOwl:id>
        <rdfs:label>Aswa County</rdfs:label>
    </owl:NamedIndividual>
    


    <!-- http://purl.obolibrary.org/obo/GAZ_00015498 -->

    <owl:NamedIndividual rdf:about="http://purl.obolibrary.org/obo/GAZ_00015498">
        <obo:RO_0001025 rdf:resource="http://purl.obolibrary.org/obo/GAZ_00009913"/>
        <obo:IAO_0000115>A county (third-level administrative division) of Uganda.</obo:IAO_0000115>
        <oboInOwl:hasOBONamespace>GAZ</oboInOwl:hasOBONamespace>
        <oboInOwl:id>GAZ:00015498</oboInOwl:id>
        <rdfs:label>Omoro County</rdfs:label>
    </owl:NamedIndividual>
    


    <!-- http://purl.obolibrary.org/obo/GAZ_00015500 -->

    <owl:NamedIndividual rdf:about="http://purl.obolibrary.org/obo/GAZ_00015500">
        <obo:RO_0001025 rdf:resource="http://purl.obolibrary.org/obo/GAZ_00015380"/>
        <obo:IAO_0000115>A county (third-level administrative division) of Uganda.</obo:IAO_0000115>
        <oboInOwl:hasOBONamespace>GAZ</oboInOwl:hasOBONamespace>
        <oboInOwl:id>GAZ:00015500</oboInOwl:id>
        <rdfs:label>Chua County</rdfs:label>
    </owl:NamedIndividual>
    


    <!-- http://purl.obolibrary.org/obo/GAZ_00015501 -->

    <owl:NamedIndividual rdf:about="http://purl.obolibrary.org/obo/GAZ_00015501">
        <obo:RO_0001025 rdf:resource="http://purl.obolibrary.org/obo/GAZ_00015380"/>
        <obo:IAO_0000115>A county (third-level administrative division) of Uganda.</obo:IAO_0000115>
        <oboInOwl:hasOBONamespace>GAZ</oboInOwl:hasOBONamespace>
        <oboInOwl:id>GAZ:00015501</oboInOwl:id>
        <rdfs:label>Lamwo County</rdfs:label>
    </owl:NamedIndividual>
    


    <!-- http://purl.obolibrary.org/obo/GAZ_00015503 -->

    <owl:NamedIndividual rdf:about="http://purl.obolibrary.org/obo/GAZ_00015503">
        <obo:RO_0001025 rdf:resource="http://purl.obolibrary.org/obo/GAZ_00015377"/>
        <obo:IAO_0000115>A county (third-level administrative division) of Uganda.</obo:IAO_0000115>
        <oboInOwl:hasOBONamespace>GAZ</oboInOwl:hasOBONamespace>
        <oboInOwl:id>GAZ:00015503</oboInOwl:id>
        <rdfs:label>Jie County</rdfs:label>
    </owl:NamedIndividual>
    


    <!-- http://purl.obolibrary.org/obo/GAZ_00015504 -->

    <owl:NamedIndividual rdf:about="http://purl.obolibrary.org/obo/GAZ_00015504">
        <rdf:type rdf:resource="http://purl.obolibrary.org/obo/ENVO_00000004"/>
        <obo:RO_0001025 rdf:resource="http://purl.obolibrary.org/obo/GAZ_00233544"/>
        <obo:IAO_0000115>A district in northeastern Uganda. Moroto District is bordered to the north by Abim District, Kotido District and Kaabong District, by the Republic of Kenya to the east, by Nakapiripirit District to the south, and to the west by Katakwi District and Amuria District.</obo:IAO_0000115>
        <oboInOwl:hasOBONamespace>GAZ</oboInOwl:hasOBONamespace>
        <oboInOwl:id>GAZ:00015504</oboInOwl:id>
        <rdfs:label>Moroto District</rdfs:label>
    </owl:NamedIndividual>
    


    <!-- http://purl.obolibrary.org/obo/GAZ_00015505 -->

    <owl:NamedIndividual rdf:about="http://purl.obolibrary.org/obo/GAZ_00015505">
        <obo:RO_0001025 rdf:resource="http://purl.obolibrary.org/obo/GAZ_00015378"/>
        <obo:IAO_0000115>A county (third-level administrative division) of Uganda.</obo:IAO_0000115>
        <oboInOwl:hasOBONamespace>GAZ</oboInOwl:hasOBONamespace>
        <oboInOwl:id>GAZ:00015505</oboInOwl:id>
        <rdfs:label>Municipality of Lira</rdfs:label>
    </owl:NamedIndividual>
    


    <!-- http://purl.obolibrary.org/obo/GAZ_00015506 -->

    <owl:NamedIndividual rdf:about="http://purl.obolibrary.org/obo/GAZ_00015506">
        <obo:RO_0001025 rdf:resource="http://purl.obolibrary.org/obo/GAZ_00015378"/>
        <obo:IAO_0000115>A county (third-level administrative division) of Uganda.</obo:IAO_0000115>
        <oboInOwl:hasOBONamespace>GAZ</oboInOwl:hasOBONamespace>
        <oboInOwl:id>GAZ:00015506</oboInOwl:id>
        <rdfs:label>Otuke County</rdfs:label>
    </owl:NamedIndividual>
    


    <!-- http://purl.obolibrary.org/obo/GAZ_00015507 -->

    <owl:NamedIndividual rdf:about="http://purl.obolibrary.org/obo/GAZ_00015507">
        <obo:RO_0001025 rdf:resource="http://purl.obolibrary.org/obo/GAZ_00015378"/>
        <obo:IAO_0000115>A county (third-level administrative division) of Uganda.</obo:IAO_0000115>
        <oboInOwl:hasOBONamespace>GAZ</oboInOwl:hasOBONamespace>
        <oboInOwl:id>GAZ:00015507</oboInOwl:id>
        <rdfs:label>Erute County</rdfs:label>
    </owl:NamedIndividual>
    


    <!-- http://purl.obolibrary.org/obo/GAZ_00015508 -->

    <owl:NamedIndividual rdf:about="http://purl.obolibrary.org/obo/GAZ_00015508">
        <obo:RO_0001025 rdf:resource="http://purl.obolibrary.org/obo/GAZ_00015386"/>
        <obo:IAO_0000115>A county (third-level administrative division) of Uganda.</obo:IAO_0000115>
        <oboInOwl:hasOBONamespace>GAZ</oboInOwl:hasOBONamespace>
        <oboInOwl:id>GAZ:00015508</oboInOwl:id>
        <rdfs:label>Maracha County</rdfs:label>
    </owl:NamedIndividual>
    


    <!-- http://purl.obolibrary.org/obo/GAZ_00015509 -->

    <owl:NamedIndividual rdf:about="http://purl.obolibrary.org/obo/GAZ_00015509">
        <obo:RO_0001025 rdf:resource="http://purl.obolibrary.org/obo/GAZ_00015386"/>
        <obo:IAO_0000115>A county (third-level administrative division) of Uganda.</obo:IAO_0000115>
        <oboInOwl:hasOBONamespace>GAZ</oboInOwl:hasOBONamespace>
        <oboInOwl:id>GAZ:00015509</oboInOwl:id>
        <rdfs:label>Terego County</rdfs:label>
    </owl:NamedIndividual>
    


    <!-- http://purl.obolibrary.org/obo/GAZ_00015510 -->

    <owl:NamedIndividual rdf:about="http://purl.obolibrary.org/obo/GAZ_00015510">
        <obo:RO_0001025 rdf:resource="http://purl.obolibrary.org/obo/GAZ_00015385"/>
        <obo:IAO_0000115>A county (third-level administrative division) of Uganda.</obo:IAO_0000115>
        <oboInOwl:hasOBONamespace>GAZ</oboInOwl:hasOBONamespace>
        <oboInOwl:id>GAZ:00015510</oboInOwl:id>
        <rdfs:label>Obongi County</rdfs:label>
    </owl:NamedIndividual>
    


    <!-- http://purl.obolibrary.org/obo/GAZ_00015511 -->

    <owl:NamedIndividual rdf:about="http://purl.obolibrary.org/obo/GAZ_00015511">
        <obo:RO_0001025 rdf:resource="http://purl.obolibrary.org/obo/GAZ_00015385"/>
        <obo:IAO_0000115>A county (third-level administrative division) of Uganda.</obo:IAO_0000115>
        <oboInOwl:hasOBONamespace>GAZ</oboInOwl:hasOBONamespace>
        <oboInOwl:id>GAZ:00015511</oboInOwl:id>
        <rdfs:label>West Moyo County</rdfs:label>
    </owl:NamedIndividual>
    


    <!-- http://purl.obolibrary.org/obo/GAZ_00015512 -->

    <owl:NamedIndividual rdf:about="http://purl.obolibrary.org/obo/GAZ_00015512">
        <obo:RO_0001025 rdf:resource="http://purl.obolibrary.org/obo/GAZ_00015383"/>
        <obo:IAO_0000115>A county (third-level administrative division) of Uganda.</obo:IAO_0000115>
        <oboInOwl:hasOBONamespace>GAZ</oboInOwl:hasOBONamespace>
        <oboInOwl:id>GAZ:00015512</oboInOwl:id>
        <rdfs:label>Chekwii County</rdfs:label>
    </owl:NamedIndividual>
    


    <!-- http://purl.obolibrary.org/obo/GAZ_00015513 -->

    <owl:NamedIndividual rdf:about="http://purl.obolibrary.org/obo/GAZ_00015513">
        <obo:RO_0001025 rdf:resource="http://purl.obolibrary.org/obo/GAZ_00015383"/>
        <obo:IAO_0000115>A county (third-level administrative division) of Uganda.</obo:IAO_0000115>
        <oboInOwl:hasOBONamespace>GAZ</oboInOwl:hasOBONamespace>
        <oboInOwl:id>GAZ:00015513</oboInOwl:id>
        <rdfs:label>Pian County</rdfs:label>
    </owl:NamedIndividual>
    


    <!-- http://purl.obolibrary.org/obo/GAZ_00015514 -->

    <owl:NamedIndividual rdf:about="http://purl.obolibrary.org/obo/GAZ_00015514">
        <obo:RO_0001025 rdf:resource="http://purl.obolibrary.org/obo/GAZ_00015375"/>
        <obo:IAO_0000115>A county (third-level administrative division) of Uganda.</obo:IAO_0000115>
        <oboInOwl:hasOBONamespace>GAZ</oboInOwl:hasOBONamespace>
        <oboInOwl:id>GAZ:00015514</oboInOwl:id>
        <rdfs:label>Okoro County</rdfs:label>
    </owl:NamedIndividual>
    


    <!-- http://purl.obolibrary.org/obo/GAZ_00015515 -->

    <owl:NamedIndividual rdf:about="http://purl.obolibrary.org/obo/GAZ_00015515">
        <obo:RO_0001025 rdf:resource="http://purl.obolibrary.org/obo/GAZ_00015375"/>
        <obo:IAO_0000115>A county (third-level administrative division) of Uganda.</obo:IAO_0000115>
        <oboInOwl:hasOBONamespace>GAZ</oboInOwl:hasOBONamespace>
        <oboInOwl:id>GAZ:00015515</oboInOwl:id>
        <rdfs:label>Jonam County</rdfs:label>
    </owl:NamedIndividual>
    


    <!-- http://purl.obolibrary.org/obo/GAZ_00015516 -->

    <owl:NamedIndividual rdf:about="http://purl.obolibrary.org/obo/GAZ_00015516">
        <obo:RO_0001025 rdf:resource="http://purl.obolibrary.org/obo/GAZ_00015375"/>
        <obo:IAO_0000115>A county (third-level administrative division) of Uganda.</obo:IAO_0000115>
        <oboInOwl:hasOBONamespace>GAZ</oboInOwl:hasOBONamespace>
        <oboInOwl:id>GAZ:00015516</oboInOwl:id>
        <rdfs:label>Padyere County</rdfs:label>
    </owl:NamedIndividual>
    


    <!-- http://purl.obolibrary.org/obo/GAZ_00015517 -->

    <owl:NamedIndividual rdf:about="http://purl.obolibrary.org/obo/GAZ_00015517">
        <obo:RO_0001025 rdf:resource="http://purl.obolibrary.org/obo/GAZ_00015379"/>
        <obo:IAO_0000115>A county (third-level administrative division) of Uganda.</obo:IAO_0000115>
        <oboInOwl:hasOBONamespace>GAZ</oboInOwl:hasOBONamespace>
        <oboInOwl:id>GAZ:00015517</oboInOwl:id>
        <rdfs:label>Oyam County</rdfs:label>
    </owl:NamedIndividual>
    


    <!-- http://purl.obolibrary.org/obo/GAZ_00015518 -->

    <owl:NamedIndividual rdf:about="http://purl.obolibrary.org/obo/GAZ_00015518">
        <obo:RO_0001025 rdf:resource="http://purl.obolibrary.org/obo/GAZ_00015381"/>
        <obo:IAO_0000115>A county (third-level administrative division) of Uganda.</obo:IAO_0000115>
        <oboInOwl:hasOBONamespace>GAZ</oboInOwl:hasOBONamespace>
        <oboInOwl:id>GAZ:00015518</oboInOwl:id>
        <rdfs:label>Agago County</rdfs:label>
    </owl:NamedIndividual>
    


    <!-- http://purl.obolibrary.org/obo/GAZ_00015519 -->

    <owl:NamedIndividual rdf:about="http://purl.obolibrary.org/obo/GAZ_00015519">
        <obo:RO_0001025 rdf:resource="http://purl.obolibrary.org/obo/GAZ_00015381"/>
        <obo:IAO_0000115>A county (third-level administrative division) of Uganda.</obo:IAO_0000115>
        <oboInOwl:hasOBONamespace>GAZ</oboInOwl:hasOBONamespace>
        <oboInOwl:id>GAZ:00015519</oboInOwl:id>
        <rdfs:label>Aruu County</rdfs:label>
    </owl:NamedIndividual>
    


    <!-- http://purl.obolibrary.org/obo/GAZ_00015520 -->

    <owl:NamedIndividual rdf:about="http://purl.obolibrary.org/obo/GAZ_00015520">
        <obo:RO_0001025 rdf:resource="http://purl.obolibrary.org/obo/GAZ_00015408"/>
        <obo:IAO_0000115>A county (third-level administrative division) of Uganda.</obo:IAO_0000115>
        <oboInOwl:hasOBONamespace>GAZ</oboInOwl:hasOBONamespace>
        <oboInOwl:id>GAZ:00015520</oboInOwl:id>
        <rdfs:label>Rubabo County</rdfs:label>
    </owl:NamedIndividual>
    


    <!-- http://purl.obolibrary.org/obo/GAZ_00015521 -->

    <owl:NamedIndividual rdf:about="http://purl.obolibrary.org/obo/GAZ_00015521">
        <obo:RO_0001025 rdf:resource="http://purl.obolibrary.org/obo/GAZ_00015408"/>
        <obo:IAO_0000115>A county (third-level administrative division) of Uganda.</obo:IAO_0000115>
        <oboInOwl:hasOBONamespace>GAZ</oboInOwl:hasOBONamespace>
        <oboInOwl:id>GAZ:00015521</oboInOwl:id>
        <rdfs:label>Rujumbura County</rdfs:label>
    </owl:NamedIndividual>
    


    <!-- http://purl.obolibrary.org/obo/GAZ_00015522 -->

    <owl:NamedIndividual rdf:about="http://purl.obolibrary.org/obo/GAZ_00015522">
        <obo:RO_0001025 rdf:resource="http://purl.obolibrary.org/obo/GAZ_00015409"/>
        <obo:IAO_0000115>A county (third-level administrative division) of Uganda.</obo:IAO_0000115>
        <oboInOwl:hasOBONamespace>GAZ</oboInOwl:hasOBONamespace>
        <oboInOwl:id>GAZ:00015522</oboInOwl:id>
        <rdfs:label>Ruhaama County</rdfs:label>
    </owl:NamedIndividual>
    


    <!-- http://purl.obolibrary.org/obo/GAZ_00015523 -->

    <owl:NamedIndividual rdf:about="http://purl.obolibrary.org/obo/GAZ_00015523">
        <obo:RO_0001025 rdf:resource="http://purl.obolibrary.org/obo/GAZ_00015409"/>
        <obo:IAO_0000115>A county (third-level administrative division) of Uganda.</obo:IAO_0000115>
        <oboInOwl:hasOBONamespace>GAZ</oboInOwl:hasOBONamespace>
        <oboInOwl:id>GAZ:00015523</oboInOwl:id>
        <rdfs:label>Kajara County</rdfs:label>
    </owl:NamedIndividual>
    


    <!-- http://purl.obolibrary.org/obo/GAZ_00015524 -->

    <owl:NamedIndividual rdf:about="http://purl.obolibrary.org/obo/GAZ_00015524">
        <obo:RO_0001025 rdf:resource="http://purl.obolibrary.org/obo/GAZ_00015409"/>
        <obo:IAO_0000115>A county (third-level administrative division) of Uganda.</obo:IAO_0000115>
        <oboInOwl:hasOBONamespace>GAZ</oboInOwl:hasOBONamespace>
        <oboInOwl:id>GAZ:00015524</oboInOwl:id>
        <rdfs:label>Rushenyi County</rdfs:label>
    </owl:NamedIndividual>
    


    <!-- http://purl.obolibrary.org/obo/GAZ_00015525 -->

    <owl:NamedIndividual rdf:about="http://purl.obolibrary.org/obo/GAZ_00015525">
        <obo:RO_0001025 rdf:resource="http://purl.obolibrary.org/obo/GAZ_00009917"/>
        <obo:IAO_0000115>A county (third-level administrative division) of Uganda.</obo:IAO_0000115>
        <oboInOwl:hasOBONamespace>GAZ</oboInOwl:hasOBONamespace>
        <oboInOwl:id>GAZ:00015525</oboInOwl:id>
        <rdfs:label>Kashari County</rdfs:label>
    </owl:NamedIndividual>
    


    <!-- http://purl.obolibrary.org/obo/GAZ_00015526 -->

    <owl:NamedIndividual rdf:about="http://purl.obolibrary.org/obo/GAZ_00015526">
        <obo:RO_0001025 rdf:resource="http://purl.obolibrary.org/obo/GAZ_00009917"/>
        <obo:IAO_0000115>A county (third-level administrative division) of Uganda.</obo:IAO_0000115>
        <oboInOwl:hasOBONamespace>GAZ</oboInOwl:hasOBONamespace>
        <oboInOwl:id>GAZ:00015526</oboInOwl:id>
        <rdfs:label>Rwampara County</rdfs:label>
    </owl:NamedIndividual>
    


    <!-- http://purl.obolibrary.org/obo/GAZ_00015527 -->

    <owl:NamedIndividual rdf:about="http://purl.obolibrary.org/obo/GAZ_00015527">
        <obo:RO_0001025 rdf:resource="http://purl.obolibrary.org/obo/GAZ_00009915"/>
        <obo:IAO_0000115>A county (third-level administrative division) of Uganda.</obo:IAO_0000115>
        <oboInOwl:hasOBONamespace>GAZ</oboInOwl:hasOBONamespace>
        <oboInOwl:id>GAZ:00015527</oboInOwl:id>
        <rdfs:label>Bujenje County</rdfs:label>
    </owl:NamedIndividual>
    


    <!-- http://purl.obolibrary.org/obo/GAZ_00015528 -->

    <owl:NamedIndividual rdf:about="http://purl.obolibrary.org/obo/GAZ_00015528">
        <obo:RO_0001025 rdf:resource="http://purl.obolibrary.org/obo/GAZ_00009915"/>
        <obo:IAO_0000115>A county (third-level administrative division) of Uganda.</obo:IAO_0000115>
        <oboInOwl:hasOBONamespace>GAZ</oboInOwl:hasOBONamespace>
        <oboInOwl:id>GAZ:00015528</oboInOwl:id>
        <rdfs:label>Kibanda County</rdfs:label>
    </owl:NamedIndividual>
    


    <!-- http://purl.obolibrary.org/obo/GAZ_00015529 -->

    <owl:NamedIndividual rdf:about="http://purl.obolibrary.org/obo/GAZ_00015529">
        <obo:RO_0001025 rdf:resource="http://purl.obolibrary.org/obo/GAZ_00009915"/>
        <obo:IAO_0000115>A county (third-level administrative division) of Uganda.</obo:IAO_0000115>
        <oboInOwl:hasOBONamespace>GAZ</oboInOwl:hasOBONamespace>
        <oboInOwl:id>GAZ:00015529</oboInOwl:id>
        <rdfs:label>Buruuli County</rdfs:label>
    </owl:NamedIndividual>
    


    <!-- http://purl.obolibrary.org/obo/GAZ_00015530 -->

    <owl:NamedIndividual rdf:about="http://purl.obolibrary.org/obo/GAZ_00015530">
        <obo:RO_0001025 rdf:resource="http://purl.obolibrary.org/obo/GAZ_00015406"/>
        <obo:IAO_0000115>A county (third-level administrative division) of Uganda.</obo:IAO_0000115>
        <oboInOwl:hasOBONamespace>GAZ</oboInOwl:hasOBONamespace>
        <oboInOwl:id>GAZ:00015530</oboInOwl:id>
        <rdfs:label>Kyaka County</rdfs:label>
    </owl:NamedIndividual>
    


    <!-- http://purl.obolibrary.org/obo/GAZ_00015531 -->

    <owl:NamedIndividual rdf:about="http://purl.obolibrary.org/obo/GAZ_00015531">
        <obo:RO_0001025 rdf:resource="http://purl.obolibrary.org/obo/GAZ_00015406"/>
        <obo:IAO_0000115>A county (third-level administrative division) of Uganda.</obo:IAO_0000115>
        <oboInOwl:hasOBONamespace>GAZ</oboInOwl:hasOBONamespace>
        <oboInOwl:id>GAZ:00015531</oboInOwl:id>
        <rdfs:label>Mwenge County</rdfs:label>
    </owl:NamedIndividual>
    


    <!-- http://purl.obolibrary.org/obo/GAZ_00015533 -->

    <owl:NamedIndividual rdf:about="http://purl.obolibrary.org/obo/GAZ_00015533">
        <obo:RO_0001025 rdf:resource="http://purl.obolibrary.org/obo/GAZ_00015407"/>
        <obo:IAO_0000115>A county (third-level administrative division) of Uganda.</obo:IAO_0000115>
        <oboInOwl:hasOBONamespace>GAZ</oboInOwl:hasOBONamespace>
        <oboInOwl:id>GAZ:00015533</oboInOwl:id>
        <rdfs:label>Kazo County</rdfs:label>
    </owl:NamedIndividual>
    


    <!-- http://purl.obolibrary.org/obo/GAZ_00015534 -->

    <owl:NamedIndividual rdf:about="http://purl.obolibrary.org/obo/GAZ_00015534">
        <obo:RO_0001025 rdf:resource="http://purl.obolibrary.org/obo/GAZ_00015407"/>
        <obo:IAO_0000115>A county (third-level administrative division) of Uganda.</obo:IAO_0000115>
        <oboInOwl:hasOBONamespace>GAZ</oboInOwl:hasOBONamespace>
        <oboInOwl:id>GAZ:00015534</oboInOwl:id>
        <rdfs:label>Nyabushozi County</rdfs:label>
    </owl:NamedIndividual>
    


    <!-- http://purl.obolibrary.org/obo/GAZ_00015535 -->

    <owl:NamedIndividual rdf:about="http://purl.obolibrary.org/obo/GAZ_00015535">
        <obo:RO_0001025 rdf:resource="http://purl.obolibrary.org/obo/GAZ_00015401"/>
        <obo:IAO_0000115>A county (third-level administrative division) of Uganda.</obo:IAO_0000115>
        <oboInOwl:hasOBONamespace>GAZ</oboInOwl:hasOBONamespace>
        <oboInOwl:id>GAZ:00015535</oboInOwl:id>
        <rdfs:label>Bugangaizi County</rdfs:label>
    </owl:NamedIndividual>
    


    <!-- http://purl.obolibrary.org/obo/GAZ_00015536 -->

    <owl:NamedIndividual rdf:about="http://purl.obolibrary.org/obo/GAZ_00015536">
        <obo:RO_0001025 rdf:resource="http://purl.obolibrary.org/obo/GAZ_00015401"/>
        <obo:IAO_0000115>A county (third-level administrative division) of Uganda.</obo:IAO_0000115>
        <oboInOwl:hasOBONamespace>GAZ</oboInOwl:hasOBONamespace>
        <oboInOwl:id>GAZ:00015536</oboInOwl:id>
        <rdfs:label>Buyaga County</rdfs:label>
    </owl:NamedIndividual>
    


    <!-- http://purl.obolibrary.org/obo/GAZ_00015537 -->

    <owl:NamedIndividual rdf:about="http://purl.obolibrary.org/obo/GAZ_00015537">
        <obo:RO_0001025 rdf:resource="http://purl.obolibrary.org/obo/GAZ_00015401"/>
        <obo:IAO_0000115>A county (third-level administrative division) of Uganda.</obo:IAO_0000115>
        <oboInOwl:hasOBONamespace>GAZ</oboInOwl:hasOBONamespace>
        <oboInOwl:id>GAZ:00015537</oboInOwl:id>
        <rdfs:label>Buyanja County</rdfs:label>
    </owl:NamedIndividual>
    


    <!-- http://purl.obolibrary.org/obo/GAZ_00015538 -->

    <owl:NamedIndividual rdf:about="http://purl.obolibrary.org/obo/GAZ_00015538">
        <obo:RO_0001025 rdf:resource="http://purl.obolibrary.org/obo/GAZ_00015394"/>
        <obo:IAO_0000115>A county (third-level administrative division) of Uganda.</obo:IAO_0000115>
        <oboInOwl:hasOBONamespace>GAZ</oboInOwl:hasOBONamespace>
        <oboInOwl:id>GAZ:00015538</oboInOwl:id>
        <rdfs:label>Bukonjo County</rdfs:label>
    </owl:NamedIndividual>
    


    <!-- http://purl.obolibrary.org/obo/GAZ_00015539 -->

    <owl:NamedIndividual rdf:about="http://purl.obolibrary.org/obo/GAZ_00015539">
        <obo:RO_0001025 rdf:resource="http://purl.obolibrary.org/obo/GAZ_00015394"/>
        <obo:IAO_0000115>A county (third-level administrative division) of Uganda.</obo:IAO_0000115>
        <oboInOwl:hasOBONamespace>GAZ</oboInOwl:hasOBONamespace>
        <oboInOwl:id>GAZ:00015539</oboInOwl:id>
        <rdfs:label>Busongora County</rdfs:label>
    </owl:NamedIndividual>
    


    <!-- http://purl.obolibrary.org/obo/GAZ_00015541 -->

    <owl:NamedIndividual rdf:about="http://purl.obolibrary.org/obo/GAZ_00015541">
        <obo:RO_0001025 rdf:resource="http://purl.obolibrary.org/obo/GAZ_00015403"/>
        <obo:IAO_0000115>A county (third-level administrative division) of Uganda.</obo:IAO_0000115>
        <oboInOwl:hasOBONamespace>GAZ</oboInOwl:hasOBONamespace>
        <oboInOwl:id>GAZ:00015541</oboInOwl:id>
        <rdfs:label>Kibale County</rdfs:label>
    </owl:NamedIndividual>
    


    <!-- http://purl.obolibrary.org/obo/GAZ_00015542 -->

    <owl:NamedIndividual rdf:about="http://purl.obolibrary.org/obo/GAZ_00015542">
        <obo:RO_0001025 rdf:resource="http://purl.obolibrary.org/obo/GAZ_00015403"/>
        <obo:IAO_0000115>A county (third-level administrative division) of Uganda.</obo:IAO_0000115>
        <oboInOwl:hasOBONamespace>GAZ</oboInOwl:hasOBONamespace>
        <oboInOwl:id>GAZ:00015542</oboInOwl:id>
        <rdfs:label>Kitagwenda County</rdfs:label>
    </owl:NamedIndividual>
    


    <!-- http://purl.obolibrary.org/obo/GAZ_00015543 -->

    <owl:NamedIndividual rdf:about="http://purl.obolibrary.org/obo/GAZ_00015543">
        <obo:RO_0001025 rdf:resource="http://purl.obolibrary.org/obo/GAZ_00015396"/>
        <obo:IAO_0000115>A county (third-level administrative division) of Uganda.</obo:IAO_0000115>
        <oboInOwl:hasOBONamespace>GAZ</oboInOwl:hasOBONamespace>
        <oboInOwl:id>GAZ:00015543</oboInOwl:id>
        <rdfs:label>Bunyangabu County</rdfs:label>
    </owl:NamedIndividual>
    


    <!-- http://purl.obolibrary.org/obo/GAZ_00015544 -->

    <owl:NamedIndividual rdf:about="http://purl.obolibrary.org/obo/GAZ_00015544">
        <obo:RO_0001025 rdf:resource="http://purl.obolibrary.org/obo/GAZ_00015396"/>
        <obo:IAO_0000115>A county (third-level administrative division) of Uganda.</obo:IAO_0000115>
        <oboInOwl:hasOBONamespace>GAZ</oboInOwl:hasOBONamespace>
        <oboInOwl:id>GAZ:00015544</oboInOwl:id>
        <rdfs:label>Burahya County</rdfs:label>
    </owl:NamedIndividual>
    


    <!-- http://purl.obolibrary.org/obo/GAZ_00015545 -->

    <owl:NamedIndividual rdf:about="http://purl.obolibrary.org/obo/GAZ_00015545">
        <obo:RO_0001025 rdf:resource="http://purl.obolibrary.org/obo/GAZ_00015396"/>
        <obo:IAO_0000115>A county (third-level administrative division) of Uganda.</obo:IAO_0000115>
        <oboInOwl:hasOBONamespace>GAZ</oboInOwl:hasOBONamespace>
        <oboInOwl:id>GAZ:00015545</oboInOwl:id>
        <rdfs:label>Municipality of Fort Portal</rdfs:label>
    </owl:NamedIndividual>
    


    <!-- http://purl.obolibrary.org/obo/GAZ_00015546 -->

    <owl:NamedIndividual rdf:about="http://purl.obolibrary.org/obo/GAZ_00015546">
        <obo:RO_0001025 rdf:resource="http://purl.obolibrary.org/obo/GAZ_00015397"/>
        <obo:IAO_0000115>A county (third-level administrative division) of Uganda.</obo:IAO_0000115>
        <oboInOwl:hasOBONamespace>GAZ</oboInOwl:hasOBONamespace>
        <oboInOwl:id>GAZ:00015546</oboInOwl:id>
        <rdfs:label>Municipality of Kabale</rdfs:label>
    </owl:NamedIndividual>
    


    <!-- http://purl.obolibrary.org/obo/GAZ_00015547 -->

    <owl:NamedIndividual rdf:about="http://purl.obolibrary.org/obo/GAZ_00015547">
        <obo:RO_0001025 rdf:resource="http://purl.obolibrary.org/obo/GAZ_00015397"/>
        <obo:IAO_0000115>A county (third-level administrative division) of Uganda.</obo:IAO_0000115>
        <oboInOwl:hasOBONamespace>GAZ</oboInOwl:hasOBONamespace>
        <oboInOwl:id>GAZ:00015547</oboInOwl:id>
        <rdfs:label>Ndorwa County</rdfs:label>
    </owl:NamedIndividual>
    


    <!-- http://purl.obolibrary.org/obo/GAZ_00015548 -->

    <owl:NamedIndividual rdf:about="http://purl.obolibrary.org/obo/GAZ_00015548">
        <obo:RO_0001025 rdf:resource="http://purl.obolibrary.org/obo/GAZ_00015397"/>
        <obo:IAO_0000115>A county (third-level administrative division) of Uganda.</obo:IAO_0000115>
        <oboInOwl:hasOBONamespace>GAZ</oboInOwl:hasOBONamespace>
        <oboInOwl:id>GAZ:00015548</oboInOwl:id>
        <rdfs:label>Rukiga County</rdfs:label>
    </owl:NamedIndividual>
    


    <!-- http://purl.obolibrary.org/obo/GAZ_00015549 -->

    <owl:NamedIndividual rdf:about="http://purl.obolibrary.org/obo/GAZ_00015549">
        <obo:RO_0001025 rdf:resource="http://purl.obolibrary.org/obo/GAZ_00015397"/>
        <obo:IAO_0000115>A county (third-level administrative division) of Uganda.</obo:IAO_0000115>
        <oboInOwl:hasOBONamespace>GAZ</oboInOwl:hasOBONamespace>
        <oboInOwl:id>GAZ:00015549</oboInOwl:id>
        <rdfs:label>Rubanda County</rdfs:label>
    </owl:NamedIndividual>
    


    <!-- http://purl.obolibrary.org/obo/GAZ_00015551 -->

    <owl:NamedIndividual rdf:about="http://purl.obolibrary.org/obo/GAZ_00015551">
        <obo:RO_0001025 rdf:resource="http://purl.obolibrary.org/obo/GAZ_00015400"/>
        <obo:IAO_0000115>A county (third-level administrative division) of Uganda.</obo:IAO_0000115>
        <oboInOwl:hasOBONamespace>GAZ</oboInOwl:hasOBONamespace>
        <oboInOwl:id>GAZ:00015551</oboInOwl:id>
        <rdfs:label>Bugahya County</rdfs:label>
    </owl:NamedIndividual>
    


    <!-- http://purl.obolibrary.org/obo/GAZ_00015552 -->

    <owl:NamedIndividual rdf:about="http://purl.obolibrary.org/obo/GAZ_00015552">
        <obo:RO_0001025 rdf:resource="http://purl.obolibrary.org/obo/GAZ_00015400"/>
        <obo:IAO_0000115>A county (third-level administrative division) of Uganda.</obo:IAO_0000115>
        <oboInOwl:hasOBONamespace>GAZ</oboInOwl:hasOBONamespace>
        <oboInOwl:id>GAZ:00015552</oboInOwl:id>
        <rdfs:label>Buhaguzi County</rdfs:label>
    </owl:NamedIndividual>
    


    <!-- http://purl.obolibrary.org/obo/GAZ_00015553 -->

    <owl:NamedIndividual rdf:about="http://purl.obolibrary.org/obo/GAZ_00015553">
        <obo:RO_0001025 rdf:resource="http://purl.obolibrary.org/obo/GAZ_00015405"/>
        <obo:IAO_0000115>A county (third-level administrative division) of Uganda.</obo:IAO_0000115>
        <oboInOwl:hasOBONamespace>GAZ</oboInOwl:hasOBONamespace>
        <oboInOwl:id>GAZ:00015553</oboInOwl:id>
        <rdfs:label>Buhweju County</rdfs:label>
    </owl:NamedIndividual>
    


    <!-- http://purl.obolibrary.org/obo/GAZ_00015554 -->

    <owl:NamedIndividual rdf:about="http://purl.obolibrary.org/obo/GAZ_00015554">
        <obo:RO_0001025 rdf:resource="http://purl.obolibrary.org/obo/GAZ_00015405"/>
        <obo:IAO_0000115>A county (third-level administrative division) of Uganda.</obo:IAO_0000115>
        <oboInOwl:hasOBONamespace>GAZ</oboInOwl:hasOBONamespace>
        <oboInOwl:id>GAZ:00015554</oboInOwl:id>
        <rdfs:label>Igara County</rdfs:label>
    </owl:NamedIndividual>
    


    <!-- http://purl.obolibrary.org/obo/GAZ_00015555 -->

    <owl:NamedIndividual rdf:about="http://purl.obolibrary.org/obo/GAZ_00015555">
        <obo:RO_0001025 rdf:resource="http://purl.obolibrary.org/obo/GAZ_00015405"/>
        <obo:IAO_0000115>A county (third-level administrative division) of Uganda.</obo:IAO_0000115>
        <oboInOwl:hasOBONamespace>GAZ</oboInOwl:hasOBONamespace>
        <oboInOwl:id>GAZ:00015555</oboInOwl:id>
        <rdfs:label>Sheema County</rdfs:label>
    </owl:NamedIndividual>
    


    <!-- http://purl.obolibrary.org/obo/GAZ_00015556 -->

    <owl:NamedIndividual rdf:about="http://purl.obolibrary.org/obo/GAZ_00015556">
        <obo:RO_0001025 rdf:resource="http://purl.obolibrary.org/obo/GAZ_00015405"/>
        <obo:IAO_0000115>A county (third-level administrative division) of Uganda.</obo:IAO_0000115>
        <oboInOwl:hasOBONamespace>GAZ</oboInOwl:hasOBONamespace>
        <oboInOwl:id>GAZ:00015556</oboInOwl:id>
        <rdfs:label>Bunyaruguru County</rdfs:label>
    </owl:NamedIndividual>
    


    <!-- http://purl.obolibrary.org/obo/GAZ_00015557 -->

    <owl:NamedIndividual rdf:about="http://purl.obolibrary.org/obo/GAZ_00015557">
        <obo:RO_0001025 rdf:resource="http://purl.obolibrary.org/obo/GAZ_00015405"/>
        <obo:IAO_0000115>A county (third-level administrative division) of Uganda.</obo:IAO_0000115>
        <oboInOwl:hasOBONamespace>GAZ</oboInOwl:hasOBONamespace>
        <oboInOwl:id>GAZ:00015557</oboInOwl:id>
        <rdfs:label>Ruhinda County</rdfs:label>
    </owl:NamedIndividual>
    


    <!-- http://purl.obolibrary.org/obo/GAZ_00015558 -->

    <owl:NamedIndividual rdf:about="http://purl.obolibrary.org/obo/GAZ_00015558">
        <obo:RO_0001025 rdf:resource="http://purl.obolibrary.org/obo/GAZ_00015402"/>
        <obo:IAO_0000115>A county (third-level administrative division) of Uganda.</obo:IAO_0000115>
        <oboInOwl:hasOBONamespace>GAZ</oboInOwl:hasOBONamespace>
        <oboInOwl:id>GAZ:00015558</oboInOwl:id>
        <rdfs:label>Bwamba County</rdfs:label>
    </owl:NamedIndividual>
    


    <!-- http://purl.obolibrary.org/obo/GAZ_00015559 -->

    <owl:NamedIndividual rdf:about="http://purl.obolibrary.org/obo/GAZ_00015559">
        <obo:RO_0001025 rdf:resource="http://purl.obolibrary.org/obo/GAZ_00015402"/>
        <obo:IAO_0000115>A county (third-level administrative division) of Uganda.</obo:IAO_0000115>
        <oboInOwl:hasOBONamespace>GAZ</oboInOwl:hasOBONamespace>
        <oboInOwl:id>GAZ:00015559</oboInOwl:id>
        <rdfs:label>Ntoroko County</rdfs:label>
    </owl:NamedIndividual>
    


    <!-- http://purl.obolibrary.org/obo/GAZ_00029996 -->

    <owl:NamedIndividual rdf:about="http://purl.obolibrary.org/obo/GAZ_00029996">
        <obo:RO_0001025 rdf:resource="http://purl.obolibrary.org/obo/GAZ_00000058"/>
        <obo:IAO_0000115>The smaller of two inhabited islands in Lake Malawi. It lies just a few km from Mozambique, and is entirely surrounded by Mozambican territorial waters, but belongs to Malawi.It is, therefore, an exclave of Malawi.</obo:IAO_0000115>
        <oboInOwl:hasOBONamespace>GAZ</oboInOwl:hasOBONamespace>
        <oboInOwl:id>GAZ:00029996</oboInOwl:id>
        <rdfs:label>Chisumulu Island</rdfs:label>
    </owl:NamedIndividual>
    


    <!-- http://purl.obolibrary.org/obo/GAZ_00029997 -->

    <owl:NamedIndividual rdf:about="http://purl.obolibrary.org/obo/GAZ_00029997">
        <obo:RO_0001025 rdf:resource="http://purl.obolibrary.org/obo/GAZ_00000058"/>
        <obo:IAO_0000115>The larger of two inhabited islands in Lake Malawi. It lies just a few km from Mozambique, and is surrounded by Mozambican territorial waters, but belongs to Malawi. An exclave of Malawi.</obo:IAO_0000115>
        <oboInOwl:hasOBONamespace>GAZ</oboInOwl:hasOBONamespace>
        <oboInOwl:id>GAZ:00029997</oboInOwl:id>
        <rdfs:label>Likoma Island</rdfs:label>
    </owl:NamedIndividual>
    


    <!-- http://purl.obolibrary.org/obo/GAZ_00040045 -->

    <owl:NamedIndividual rdf:about="http://purl.obolibrary.org/obo/GAZ_00040045">
        <obo:RO_0001025 rdf:resource="http://purl.obolibrary.org/obo/GAZ_00015344"/>
        <obo:RO_0001025 rdf:resource="http://purl.obolibrary.org/obo/GAZ_00015452"/>
        <obo:IAO_0000115>An archipelago of eighty-four islands in the northwest of Lake Victoria, Uganda. The islands lie in two main groups, separated by the Kkome Channel.</obo:IAO_0000115>
        <oboInOwl:hasOBONamespace>GAZ</oboInOwl:hasOBONamespace>
        <oboInOwl:id>GAZ:00040045</oboInOwl:id>
        <rdfs:label>Ssese Islands</rdfs:label>
    </owl:NamedIndividual>
    


    <!-- http://purl.obolibrary.org/obo/GAZ_00040046 -->

    <owl:NamedIndividual rdf:about="http://purl.obolibrary.org/obo/GAZ_00040046">
        <obo:RO_0001025 rdf:resource="http://purl.obolibrary.org/obo/GAZ_00040045"/>
        <oboInOwl:hasOBONamespace>GAZ</oboInOwl:hasOBONamespace>
        <oboInOwl:id>GAZ:00040046</oboInOwl:id>
        <rdfs:label>Northeast Ssese Islands</rdfs:label>
    </owl:NamedIndividual>
    


    <!-- http://purl.obolibrary.org/obo/GAZ_00040047 -->

    <owl:NamedIndividual rdf:about="http://purl.obolibrary.org/obo/GAZ_00040047">
        <obo:RO_0001025 rdf:resource="http://purl.obolibrary.org/obo/GAZ_00040045"/>
        <oboInOwl:hasOBONamespace>GAZ</oboInOwl:hasOBONamespace>
        <oboInOwl:id>GAZ:00040047</oboInOwl:id>
        <rdfs:label>Southwest Ssese Islands</rdfs:label>
    </owl:NamedIndividual>
    


    <!-- http://purl.obolibrary.org/obo/GAZ_00040048 -->

    <owl:NamedIndividual rdf:about="http://purl.obolibrary.org/obo/GAZ_00040048">
        <obo:RO_0001025 rdf:resource="http://purl.obolibrary.org/obo/GAZ_00040046"/>
        <oboInOwl:hasOBONamespace>GAZ</oboInOwl:hasOBONamespace>
        <oboInOwl:id>GAZ:00040048</oboInOwl:id>
        <rdfs:label>Damba Island</rdfs:label>
    </owl:NamedIndividual>
    


    <!-- http://purl.obolibrary.org/obo/GAZ_00040049 -->

    <owl:NamedIndividual rdf:about="http://purl.obolibrary.org/obo/GAZ_00040049">
        <obo:RO_0001025 rdf:resource="http://purl.obolibrary.org/obo/GAZ_00040046"/>
        <oboInOwl:hasOBONamespace>GAZ</oboInOwl:hasOBONamespace>
        <oboInOwl:id>GAZ:00040049</oboInOwl:id>
        <rdfs:label>Kkome Island</rdfs:label>
    </owl:NamedIndividual>
    


    <!-- http://purl.obolibrary.org/obo/GAZ_00040050 -->

    <owl:NamedIndividual rdf:about="http://purl.obolibrary.org/obo/GAZ_00040050">
        <obo:RO_0001025 rdf:resource="http://purl.obolibrary.org/obo/GAZ_00040046"/>
        <oboInOwl:hasOBONamespace>GAZ</oboInOwl:hasOBONamespace>
        <oboInOwl:id>GAZ:00040050</oboInOwl:id>
        <rdfs:label>Luwaji Island</rdfs:label>
    </owl:NamedIndividual>
    


    <!-- http://purl.obolibrary.org/obo/GAZ_00040051 -->

    <owl:NamedIndividual rdf:about="http://purl.obolibrary.org/obo/GAZ_00040051">
        <obo:RO_0001025 rdf:resource="http://purl.obolibrary.org/obo/GAZ_00040047"/>
        <oboInOwl:hasOBONamespace>GAZ</oboInOwl:hasOBONamespace>
        <oboInOwl:id>GAZ:00040051</oboInOwl:id>
        <rdfs:label>Buyova Island</rdfs:label>
    </owl:NamedIndividual>
    


    <!-- http://purl.obolibrary.org/obo/GAZ_00040052 -->

    <owl:NamedIndividual rdf:about="http://purl.obolibrary.org/obo/GAZ_00040052">
        <obo:RO_0001025 rdf:resource="http://purl.obolibrary.org/obo/GAZ_00040047"/>
        <oboInOwl:hasOBONamespace>GAZ</oboInOwl:hasOBONamespace>
        <oboInOwl:id>GAZ:00040052</oboInOwl:id>
        <rdfs:label>Serinya Island</rdfs:label>
    </owl:NamedIndividual>
    


    <!-- http://purl.obolibrary.org/obo/GAZ_00040053 -->

    <owl:NamedIndividual rdf:about="http://purl.obolibrary.org/obo/GAZ_00040053">
        <obo:RO_0001025 rdf:resource="http://purl.obolibrary.org/obo/GAZ_00040047"/>
        <oboInOwl:hasOBONamespace>GAZ</oboInOwl:hasOBONamespace>
        <oboInOwl:id>GAZ:00040053</oboInOwl:id>
        <rdfs:label>Funve Island</rdfs:label>
    </owl:NamedIndividual>
    


    <!-- http://purl.obolibrary.org/obo/GAZ_00040054 -->

    <owl:NamedIndividual rdf:about="http://purl.obolibrary.org/obo/GAZ_00040054">
        <obo:RO_0001025 rdf:resource="http://purl.obolibrary.org/obo/GAZ_00040047"/>
        <obo:IAO_0000115>The second largest island in Lake Victoria, Uganda, after Ukerewe. Its area is 275 km2. It is a part of the Ssese Islands in the Kalangala District. Chief town is Kalangala.</obo:IAO_0000115>
        <oboInOwl:hasOBONamespace>GAZ</oboInOwl:hasOBONamespace>
        <oboInOwl:id>GAZ:00040054</oboInOwl:id>
        <rdfs:label>Bugala Island</rdfs:label>
    </owl:NamedIndividual>
    


    <!-- http://purl.obolibrary.org/obo/GAZ_00040055 -->

    <owl:NamedIndividual rdf:about="http://purl.obolibrary.org/obo/GAZ_00040055">
        <obo:RO_0001025 rdf:resource="http://purl.obolibrary.org/obo/GAZ_00040047"/>
        <oboInOwl:hasOBONamespace>GAZ</oboInOwl:hasOBONamespace>
        <oboInOwl:id>GAZ:00040055</oboInOwl:id>
        <rdfs:label>Bufumira Island</rdfs:label>
    </owl:NamedIndividual>
    


    <!-- http://purl.obolibrary.org/obo/GAZ_00040056 -->

    <owl:NamedIndividual rdf:about="http://purl.obolibrary.org/obo/GAZ_00040056">
        <obo:RO_0001025 rdf:resource="http://purl.obolibrary.org/obo/GAZ_00040047"/>
        <oboInOwl:hasOBONamespace>GAZ</oboInOwl:hasOBONamespace>
        <oboInOwl:id>GAZ:00040056</oboInOwl:id>
        <rdfs:label>Bukasa Island</rdfs:label>
    </owl:NamedIndividual>
    


    <!-- http://purl.obolibrary.org/obo/GAZ_00040057 -->

    <owl:NamedIndividual rdf:about="http://purl.obolibrary.org/obo/GAZ_00040057">
        <obo:RO_0001025 rdf:resource="http://purl.obolibrary.org/obo/GAZ_00040047"/>
        <oboInOwl:hasOBONamespace>GAZ</oboInOwl:hasOBONamespace>
        <oboInOwl:id>GAZ:00040057</oboInOwl:id>
        <rdfs:label>Bugaba Island</rdfs:label>
    </owl:NamedIndividual>
    


    <!-- http://purl.obolibrary.org/obo/GAZ_00040058 -->

    <owl:NamedIndividual rdf:about="http://purl.obolibrary.org/obo/GAZ_00040058">
        <obo:RO_0001025 rdf:resource="http://purl.obolibrary.org/obo/GAZ_00040047"/>
        <oboInOwl:hasOBONamespace>GAZ</oboInOwl:hasOBONamespace>
        <oboInOwl:id>GAZ:00040058</oboInOwl:id>
        <rdfs:label>Bubeke Island</rdfs:label>
    </owl:NamedIndividual>
    


    <!-- http://purl.obolibrary.org/obo/GAZ_00041527 -->

    <owl:NamedIndividual rdf:about="http://purl.obolibrary.org/obo/GAZ_00041527">
        <obo:RO_0001025 rdf:resource="http://purl.obolibrary.org/obo/GAZ_00015452"/>
        <obo:IAO_0000115>The largest island in Lake Victoria, the largest inland island in Africa. Located 45 km north of Mwanza.</obo:IAO_0000115>
        <oboInOwl:hasOBONamespace>GAZ</oboInOwl:hasOBONamespace>
        <oboInOwl:id>GAZ:00041527</oboInOwl:id>
        <rdfs:label>Ukerewe Island</rdfs:label>
    </owl:NamedIndividual>
    


    <!-- http://purl.obolibrary.org/obo/GAZ_00041528 -->

    <owl:NamedIndividual rdf:about="http://purl.obolibrary.org/obo/GAZ_00041528">
        <obo:RO_0001025 rdf:resource="http://purl.obolibrary.org/obo/GAZ_00000007"/>
        <obo:IAO_0000115>An endorheic lake, in western Zomba District of Malawi, near the border with Mozambique.</obo:IAO_0000115>
        <oboInOwl:hasOBONamespace>GAZ</oboInOwl:hasOBONamespace>
        <oboInOwl:id>GAZ:00041528</oboInOwl:id>
        <rdfs:label>Lake Chilwa</rdfs:label>
    </owl:NamedIndividual>
    


    <!-- http://purl.obolibrary.org/obo/GAZ_00041529 -->

    <owl:NamedIndividual rdf:about="http://purl.obolibrary.org/obo/GAZ_00041529">
        <obo:RO_0001025 rdf:resource="http://purl.obolibrary.org/obo/GAZ_00000007"/>
        <obo:IAO_0000115>A lake in southern part of Malawi, in the Southern Region.</obo:IAO_0000115>
        <oboInOwl:hasOBONamespace>GAZ</oboInOwl:hasOBONamespace>
        <oboInOwl:id>GAZ:00041529</oboInOwl:id>
        <rdfs:label>Lake Malombe</rdfs:label>
    </owl:NamedIndividual>
    


    <!-- http://purl.obolibrary.org/obo/GAZ_00041530 -->

    <owl:NamedIndividual rdf:about="http://purl.obolibrary.org/obo/GAZ_00041530">
        <obo:RO_0001025 rdf:resource="http://purl.obolibrary.org/obo/GAZ_00000007"/>
        <obo:IAO_0000115>A freshwater lake on the longest arm of Africa&apos;s second-longest river, the Congo. Located on the border between Zambia and Democratic Republic of the Congo, it makes up 110 km of the total length of the Congo, lying between its Luapula River (upstream) and Luvua River (downstream) segments. Mweru is mainly fed by the Luapula River, which comes in through swamps from the south, and the Kalungwishi River from the east. At its north end the lake is drained by the Luvua River, which flows in a northwesterly direction to join the Lualaba River and thence to the Congo.</obo:IAO_0000115>
        <oboInOwl:hasOBONamespace>GAZ</oboInOwl:hasOBONamespace>
        <oboInOwl:id>GAZ:00041530</oboInOwl:id>
        <rdfs:label>Lake Mweru</rdfs:label>
    </owl:NamedIndividual>
    


    <!-- http://purl.obolibrary.org/obo/GAZ_00041531 -->

    <owl:NamedIndividual rdf:about="http://purl.obolibrary.org/obo/GAZ_00041531">
        <obo:RO_0001025 rdf:resource="http://purl.obolibrary.org/obo/GAZ_00000007"/>
        <obo:IAO_0000115>An alkaline lake in southwestern Tanzania. It is divided into two basins by a central swamp zone, ranging from 5-20 km wide. It is fed by 17 rivers. Seven rivers enter the south basin and 10 discharge to the north basin.</obo:IAO_0000115>
        <oboInOwl:hasOBONamespace>GAZ</oboInOwl:hasOBONamespace>
        <oboInOwl:id>GAZ:00041531</oboInOwl:id>
        <rdfs:label>Lake Rukwa</rdfs:label>
    </owl:NamedIndividual>
    


    <!-- http://purl.obolibrary.org/obo/GAZ_00041532 -->

    <owl:NamedIndividual rdf:about="http://purl.obolibrary.org/obo/GAZ_00041532">
        <obo:RO_0001025 rdf:resource="http://purl.obolibrary.org/obo/GAZ_00000007"/>
        <obo:IAO_0000115>An endorheic lake and swamp system in the Northern Province of Zambia. A rift valley lake lying in a branch of the Great Rift Valley, running from the Luapula River to Lake Tanganyika. There are some hot springs characteristics of a rift valley to the east. Its water is muddy in appearance, at times appearing reddish and &apos;slightly oily&apos;.</obo:IAO_0000115>
        <oboInOwl:hasOBONamespace>GAZ</oboInOwl:hasOBONamespace>
        <oboInOwl:id>GAZ:00041532</oboInOwl:id>
        <rdfs:label>Lake Mweru Wantipa</rdfs:label>
    </owl:NamedIndividual>
    


    <!-- http://purl.obolibrary.org/obo/GAZ_00041533 -->

    <owl:NamedIndividual rdf:about="http://purl.obolibrary.org/obo/GAZ_00041533">
        <obo:RO_0001025 rdf:resource="http://purl.obolibrary.org/obo/GAZ_00000007"/>
        <obo:IAO_0000115>A lake located in the western Great Rift Valley, on the border between the Democratic Republic of the Congo and Uganda, with its northern shore a few km south of the Equator. Lake Edward lies at an elevation of 920 metres, is 77 km long by 40 km wide at its maximum points, and covers a total surface area of 2,325 km2 (the 15th largest on the continent). The lake is fed by the Nyamugasani, the Ishasha, the Rutshuru, and the Rwindi rivers. It empties to the north via the Semliki River into Lake Albert. Lake George to the northeast empties into Lake Edward via the Kazinga Channel.</obo:IAO_0000115>
        <oboInOwl:hasOBONamespace>GAZ</oboInOwl:hasOBONamespace>
        <oboInOwl:id>GAZ:00041533</oboInOwl:id>
        <rdfs:label>Lake Edward</rdfs:label>
    </owl:NamedIndividual>
    


    <!-- http://purl.obolibrary.org/obo/GAZ_00041534 -->

    <owl:NamedIndividual rdf:about="http://purl.obolibrary.org/obo/GAZ_00041534">
        <obo:RO_0001025 rdf:resource="http://purl.obolibrary.org/obo/GAZ_00000007"/>
        <obo:IAO_0000115>A monomictic freshwater lake located in the center of the continent, on the border between Uganda and the Democratic Republic of the Congo (formerly Zaire). Lake Albert is the northernmost of the chain of lakes in the Great Rift Valley; it is about 160 km long and 30 km wide, with a maximum depth of 51 m, and a surface elevation of 619 m above sea level. Lake Albert is part of the complicated system of the upper Nile. Its main sources are the Victoria Nile, ultimately coming from Lake Victoria to the southeast, and the Semliki River, which issues from Lake Edward to the southwest. The water of the Victoria Nile is much less saline than that of Lake Albert. Its outlet, at the northernmost tip of the lake, is the Albert Nile (which becomes known as the Mountain Nile when it enters Sudan).</obo:IAO_0000115>
        <oboInOwl:hasOBONamespace>GAZ</oboInOwl:hasOBONamespace>
        <oboInOwl:id>GAZ:00041534</oboInOwl:id>
        <rdfs:label>Lake Albert</rdfs:label>
    </owl:NamedIndividual>
    


    <!-- http://purl.obolibrary.org/obo/GAZ_00041535 -->

    <owl:NamedIndividual rdf:about="http://purl.obolibrary.org/obo/GAZ_00041535">
        <rdf:type rdf:resource="http://purl.obolibrary.org/obo/ENVO_00000019"/>
        <obo:RO_0001025 rdf:resource="http://purl.obolibrary.org/obo/GAZ_00000007"/>
        <obo:IAO_0000115>A soda lake located in northern Tanzania, close to the Kenyan border, in Africa&apos;s Great Rift Valley. The lake is quite shallow, less than three m deep, and varies in width depending on its water level.</obo:IAO_0000115>
        <oboInOwl:hasOBONamespace>GAZ</oboInOwl:hasOBONamespace>
        <oboInOwl:id>GAZ:00041535</oboInOwl:id>
        <rdfs:label>Lake Natron</rdfs:label>
    </owl:NamedIndividual>
    


    <!-- http://purl.obolibrary.org/obo/GAZ_00041536 -->

    <owl:NamedIndividual rdf:about="http://purl.obolibrary.org/obo/GAZ_00041536">
        <obo:RO_0001025 rdf:resource="http://purl.obolibrary.org/obo/GAZ_00000007"/>
        <obo:RO_0001025 rdf:resource="http://purl.obolibrary.org/obo/GAZ_00136138"/>
        <obo:IAO_0000115>An endorheic soda lake located south of the Serengeti National Park and immediately southwest of the Ngorongoro Crater in the Crater Highlands area of Tanzania.</obo:IAO_0000115>
        <oboInOwl:hasOBONamespace>GAZ</oboInOwl:hasOBONamespace>
        <oboInOwl:id>GAZ:00041536</oboInOwl:id>
        <rdfs:label>Lake Eyasi</rdfs:label>
    </owl:NamedIndividual>
    


    <!-- http://purl.obolibrary.org/obo/GAZ_00041537 -->

    <owl:NamedIndividual rdf:about="http://purl.obolibrary.org/obo/GAZ_00041537">
        <obo:RO_0001025 rdf:resource="http://purl.obolibrary.org/obo/GAZ_00000007"/>
        <obo:IAO_0000115>A holopolymictic freshwater lake in Kenya, lying north west of Nairobi, outside the town of Naivasha. It is part of the Great Rift Valley. A Ramsar Site.</obo:IAO_0000115>
        <oboInOwl:hasOBONamespace>GAZ</oboInOwl:hasOBONamespace>
        <oboInOwl:id>GAZ:00041537</oboInOwl:id>
        <rdfs:label>Lake Naivasha</rdfs:label>
    </owl:NamedIndividual>
    


    <!-- http://purl.obolibrary.org/obo/GAZ_00041538 -->

    <owl:NamedIndividual rdf:about="http://purl.obolibrary.org/obo/GAZ_00041538">
        <obo:RO_0001025 rdf:resource="http://purl.obolibrary.org/obo/GAZ_00000007"/>
        <obo:IAO_0000115>A monomictic alkaline endorheic lake.</obo:IAO_0000115>
        <oboInOwl:hasOBONamespace>GAZ</oboInOwl:hasOBONamespace>
        <oboInOwl:id>GAZ:00041538</oboInOwl:id>
        <rdfs:label>Lake Turkana</rdfs:label>
    </owl:NamedIndividual>
    


    <!-- http://purl.obolibrary.org/obo/GAZ_00041539 -->

    <owl:NamedIndividual rdf:about="http://purl.obolibrary.org/obo/GAZ_00041539">
        <obo:RO_0001025 rdf:resource="http://purl.obolibrary.org/obo/GAZ_00000007"/>
        <obo:IAO_0000115>A freshwater lake fed by several rivers. It has no obvious outlet; the waters seep into lava. A Ramsar Site.</obo:IAO_0000115>
        <oboInOwl:hasOBONamespace>GAZ</oboInOwl:hasOBONamespace>
        <oboInOwl:id>GAZ:00041539</oboInOwl:id>
        <rdfs:label>Lake Baringo</rdfs:label>
    </owl:NamedIndividual>
    


    <!-- http://purl.obolibrary.org/obo/GAZ_00041540 -->

    <owl:NamedIndividual rdf:about="http://purl.obolibrary.org/obo/GAZ_00041540">
        <obo:RO_0001025 rdf:resource="http://purl.obolibrary.org/obo/GAZ_00000007"/>
        <obo:RO_0001025 rdf:resource="http://purl.obolibrary.org/obo/GAZ_00236097"/>
        <obo:IAO_0000115>A saline, alkaline lake that lies at the northern end of the arid Suguta Valley in the northern Kenya Rift. It is separated from Lake Turkana by the Barrier volcanic complex, a group of young volcanoes that last erupted during the late 19th Century or early 20th Century. Saline hot springs discharge on the northern shoreline of Lake Logipi and at Cathedral Rocks near its southern limit, and help to maintain water at times of extreme aridity. During the rainy season, the lake is also recharged from the Suguta River which flows northward along the Suguta Valley, periodically forming a temporary lake (Lake Alablab) that unites with Logipi.</obo:IAO_0000115>
        <oboInOwl:hasOBONamespace>GAZ</oboInOwl:hasOBONamespace>
        <oboInOwl:id>GAZ:00041540</oboInOwl:id>
        <rdfs:label>Lake Logipi</rdfs:label>
    </owl:NamedIndividual>
    


    <!-- http://purl.obolibrary.org/obo/GAZ_00041541 -->

    <owl:NamedIndividual rdf:about="http://purl.obolibrary.org/obo/GAZ_00041541">
        <obo:RO_0001025 rdf:resource="http://purl.obolibrary.org/obo/GAZ_00041539"/>
        <obo:IAO_0000115>An Island in the center of Lake Baringo SW of Korosi volcano consists of young basaltic scoria cones that cap a trachytic shield volcano. The volcano is the smallest in the northern part of the Kenya rift valley. N-S-trending faults cut the complex, producing west-facing scarps. Smaller islands to the north and south are faulted basaltic lava flows; Parmalok Island to the SW is a breached trachytic tuff cone that fed a small lava flow. Hot springs, boiling mud pools, and fumaroles are present along the faults on the NE peninsula of the island.</obo:IAO_0000115>
        <oboInOwl:hasOBONamespace>GAZ</oboInOwl:hasOBONamespace>
        <oboInOwl:id>GAZ:00041541</oboInOwl:id>
        <rdfs:label>Ol Kokwe Island</rdfs:label>
    </owl:NamedIndividual>
    


    <!-- http://purl.obolibrary.org/obo/GAZ_00041542 -->

    <owl:NamedIndividual rdf:about="http://purl.obolibrary.org/obo/GAZ_00041542">
        <obo:RO_0001025 rdf:resource="http://purl.obolibrary.org/obo/GAZ_00041538"/>
        <obo:IAO_0000115>The northernmost and smallest of three volcanic islands in the Lake Turkana. North Island is the summit of Kenya&apos;s northernmost rift valley volcano and is primarily composed of trachyandesitic-to-trachytic phreatomagmatic deposits from overlapping eroded tuff cones or tuff rings. The center of the island consists of a young tuff ring about 1 km in diameter nested inside an older tuff ring. Two fresh unvegetated lava flows that reach the lake shore from the central tuff ring form lava deltas at the northern and western sides of the island; the northern delta is about 900 m wide.</obo:IAO_0000115>
        <oboInOwl:hasOBONamespace>GAZ</oboInOwl:hasOBONamespace>
        <oboInOwl:id>GAZ:00041542</oboInOwl:id>
        <rdfs:label>North Island</rdfs:label>
    </owl:NamedIndividual>
    


    <!-- http://purl.obolibrary.org/obo/GAZ_00041543 -->

    <owl:NamedIndividual rdf:about="http://purl.obolibrary.org/obo/GAZ_00041543">
        <obo:RO_0001025 rdf:resource="http://purl.obolibrary.org/obo/GAZ_00041538"/>
        <obo:IAO_0000115>An island that occupies the middle of Lake Turkana and is composed of more than a dozen craters and cones, three of which are filled by small lakes. The two largest lakes partially fill craters up to a km wide and about 80 m deep whose floors lie near sea level. The highest point on the dominantly basaltic island reaches 550 m, about 170 m above the lake surface. An E-W-trending chain of small explosion craters cuts the eastern side of the 3 km wide island. Several small islands to the SE represent partially submerged crater rims, and other cones and lava plugs lie beneath the lake surface near the island.</obo:IAO_0000115>
        <oboInOwl:hasOBONamespace>GAZ</oboInOwl:hasOBONamespace>
        <oboInOwl:id>GAZ:00041543</oboInOwl:id>
        <rdfs:label>Central Island</rdfs:label>
    </owl:NamedIndividual>
    


    <!-- http://purl.obolibrary.org/obo/GAZ_00041544 -->

    <owl:NamedIndividual rdf:about="http://purl.obolibrary.org/obo/GAZ_00041544">
        <obo:RO_0001025 rdf:resource="http://purl.obolibrary.org/obo/GAZ_00041538"/>
        <obo:IAO_0000115>An island that contains numerous tuff cones. Fresh-looking lava flows, erupted from a N-S fissure extending the 11 km length of the island, form much of the eastern shoreline. South Island rises 320 m above the lake to a height of 800 m and is part of a volcanic horst that extends 10 km to the north beneath the lake surface.</obo:IAO_0000115>
        <oboInOwl:hasOBONamespace>GAZ</oboInOwl:hasOBONamespace>
        <oboInOwl:id>GAZ:00041544</oboInOwl:id>
        <rdfs:label>South Island</rdfs:label>
    </owl:NamedIndividual>
    


    <!-- http://purl.obolibrary.org/obo/GAZ_00041545 -->

    <owl:NamedIndividual rdf:about="http://purl.obolibrary.org/obo/GAZ_00041545">
        <obo:RO_0001025 rdf:resource="http://purl.obolibrary.org/obo/GAZ_00041530"/>
        <obo:IAO_0000115>An island in Lake Mweru.</obo:IAO_0000115>
        <oboInOwl:hasOBONamespace>GAZ</oboInOwl:hasOBONamespace>
        <oboInOwl:id>GAZ:00041545</oboInOwl:id>
        <rdfs:label>Kilwa Island</rdfs:label>
    </owl:NamedIndividual>
    


    <!-- http://purl.obolibrary.org/obo/GAZ_00041546 -->

    <owl:NamedIndividual rdf:about="http://purl.obolibrary.org/obo/GAZ_00041546">
        <obo:RO_0001025 rdf:resource="http://purl.obolibrary.org/obo/GAZ_00041530"/>
        <oboInOwl:hasOBONamespace>GAZ</oboInOwl:hasOBONamespace>
        <oboInOwl:id>GAZ:00041546</oboInOwl:id>
        <rdfs:label>Isokwe Island</rdfs:label>
    </owl:NamedIndividual>
    


    <!-- http://purl.obolibrary.org/obo/GAZ_00041547 -->

    <owl:NamedIndividual rdf:about="http://purl.obolibrary.org/obo/GAZ_00041547">
        <obo:RO_0001025 rdf:resource="http://purl.obolibrary.org/obo/GAZ_00041534"/>
        <oboInOwl:hasOBONamespace>GAZ</oboInOwl:hasOBONamespace>
        <oboInOwl:id>GAZ:00041547</oboInOwl:id>
        <rdfs:label>Rukwanzi Island</rdfs:label>
    </owl:NamedIndividual>
    


    <!-- http://purl.obolibrary.org/obo/GAZ_00041548 -->

    <owl:NamedIndividual rdf:about="http://purl.obolibrary.org/obo/GAZ_00041548">
        <obo:RO_0001025 rdf:resource="http://purl.obolibrary.org/obo/GAZ_00041537"/>
        <obo:IAO_0000115>An island of Lake Naivasha.</obo:IAO_0000115>
        <oboInOwl:hasOBONamespace>GAZ</oboInOwl:hasOBONamespace>
        <oboInOwl:id>GAZ:00041548</oboInOwl:id>
        <rdfs:label>Crescent Island</rdfs:label>
    </owl:NamedIndividual>
    


    <!-- http://purl.obolibrary.org/obo/GAZ_00041549 -->

    <owl:NamedIndividual rdf:about="http://purl.obolibrary.org/obo/GAZ_00041549">
        <obo:RO_0001025 rdf:resource="http://purl.obolibrary.org/obo/GAZ_00053591"/>
        <obo:IAO_0000115>A polymictic soda lake. A Ramsar Site.</obo:IAO_0000115>
        <oboInOwl:hasOBONamespace>GAZ</oboInOwl:hasOBONamespace>
        <oboInOwl:id>GAZ:00041549</oboInOwl:id>
        <rdfs:label>Lake Nakuru</rdfs:label>
    </owl:NamedIndividual>
    


    <!-- http://purl.obolibrary.org/obo/GAZ_00041550 -->

    <owl:NamedIndividual rdf:about="http://purl.obolibrary.org/obo/GAZ_00041550">
        <obo:RO_0001025 rdf:resource="http://purl.obolibrary.org/obo/GAZ_00000007"/>
        <obo:IAO_0000115>A lake that is the source of the Blue Nile and is the largest lake in Ethiopia. Located in the north-western Ethiopian highlands. Lake Tana is fed by the Little Abay, Reb and Gumara Rivers.</obo:IAO_0000115>
        <oboInOwl:hasOBONamespace>GAZ</oboInOwl:hasOBONamespace>
        <oboInOwl:id>GAZ:00041550</oboInOwl:id>
        <rdfs:label>Lake Tana</rdfs:label>
    </owl:NamedIndividual>
    


    <!-- http://purl.obolibrary.org/obo/GAZ_00041551 -->

    <owl:NamedIndividual rdf:about="http://purl.obolibrary.org/obo/GAZ_00041551">
        <obo:RO_0001025 rdf:resource="http://purl.obolibrary.org/obo/GAZ_00041550"/>
        <obo:IAO_0000115>An island in Lake Tana in Ethiopia.</obo:IAO_0000115>
        <oboInOwl:hasOBONamespace>GAZ</oboInOwl:hasOBONamespace>
        <oboInOwl:id>GAZ:00041551</oboInOwl:id>
        <rdfs:label>Tana Qirqos Island</rdfs:label>
    </owl:NamedIndividual>
    


    <!-- http://purl.obolibrary.org/obo/GAZ_00041552 -->

    <owl:NamedIndividual rdf:about="http://purl.obolibrary.org/obo/GAZ_00041552">
        <obo:RO_0001025 rdf:resource="http://purl.obolibrary.org/obo/GAZ_00041550"/>
        <obo:IAO_0000115>An island of Lake Tana.</obo:IAO_0000115>
        <oboInOwl:hasOBONamespace>GAZ</oboInOwl:hasOBONamespace>
        <oboInOwl:id>GAZ:00041552</oboInOwl:id>
        <rdfs:label>Meshralia Island</rdfs:label>
    </owl:NamedIndividual>
    


    <!-- http://purl.obolibrary.org/obo/GAZ_00041553 -->

    <owl:NamedIndividual rdf:about="http://purl.obolibrary.org/obo/GAZ_00041553">
        <obo:RO_0001025 rdf:resource="http://purl.obolibrary.org/obo/GAZ_00041550"/>
        <obo:IAO_0000115>An island of Lake Tana.</obo:IAO_0000115>
        <oboInOwl:hasOBONamespace>GAZ</oboInOwl:hasOBONamespace>
        <oboInOwl:id>GAZ:00041553</oboInOwl:id>
        <rdfs:label>Daga Island</rdfs:label>
    </owl:NamedIndividual>
    


    <!-- http://purl.obolibrary.org/obo/GAZ_00041554 -->

    <owl:NamedIndividual rdf:about="http://purl.obolibrary.org/obo/GAZ_00041554">
        <obo:RO_0001025 rdf:resource="http://purl.obolibrary.org/obo/GAZ_00041550"/>
        <obo:IAO_0000115>The biggest island (approximately 16 km2) on Lake Tana in Ethiopia. It is administratively included in the Achefer woreda of the Mirab Gojjam Zone.</obo:IAO_0000115>
        <oboInOwl:hasOBONamespace>GAZ</oboInOwl:hasOBONamespace>
        <oboInOwl:id>GAZ:00041554</oboInOwl:id>
        <rdfs:label>Dek Island</rdfs:label>
    </owl:NamedIndividual>
    


    <!-- http://purl.obolibrary.org/obo/GAZ_00041555 -->

    <owl:NamedIndividual rdf:about="http://purl.obolibrary.org/obo/GAZ_00041555">
        <obo:RO_0001025 rdf:resource="http://purl.obolibrary.org/obo/GAZ_00000007"/>
        <obo:IAO_0000115>A freshwater Rift Valley lake of Ethiopia. It is located about 60 miles south of Addis Ababa, on the border between the regions (or kililoch) of Oromia and of the Southern Nations, Nationalities, and Peoples. The lake is fed primarily by two rivers, the Meki and the Katar, but does not always have an outflow, although in some years it drains into Lake Abijatta.</obo:IAO_0000115>
        <oboInOwl:hasOBONamespace>GAZ</oboInOwl:hasOBONamespace>
        <oboInOwl:id>GAZ:00041555</oboInOwl:id>
        <rdfs:label>Lake Zway</rdfs:label>
    </owl:NamedIndividual>
    


    <!-- http://purl.obolibrary.org/obo/GAZ_00041556 -->

    <owl:NamedIndividual rdf:about="http://purl.obolibrary.org/obo/GAZ_00041556">
        <obo:RO_0001025 rdf:resource="http://purl.obolibrary.org/obo/GAZ_00000007"/>
        <obo:IAO_0000115>A polymictic freshwater lake in Ethiopia, located in the Rift Valley south of Addis Ababa. Thought to have a subterranean outlet.</obo:IAO_0000115>
        <oboInOwl:hasOBONamespace>GAZ</oboInOwl:hasOBONamespace>
        <oboInOwl:id>GAZ:00041556</oboInOwl:id>
        <rdfs:label>Lake Awasa</rdfs:label>
    </owl:NamedIndividual>
    


    <!-- http://purl.obolibrary.org/obo/GAZ_00041557 -->

    <owl:NamedIndividual rdf:about="http://purl.obolibrary.org/obo/GAZ_00041557">
        <obo:RO_0001025 rdf:resource="http://purl.obolibrary.org/obo/GAZ_00000007"/>
        <obo:IAO_0000115>A lake in Ethiopia.</obo:IAO_0000115>
        <oboInOwl:hasOBONamespace>GAZ</oboInOwl:hasOBONamespace>
        <oboInOwl:id>GAZ:00041557</oboInOwl:id>
        <rdfs:label>Lake Koka</rdfs:label>
    </owl:NamedIndividual>
    


    <!-- http://purl.obolibrary.org/obo/GAZ_00041559 -->

    <owl:NamedIndividual rdf:about="http://purl.obolibrary.org/obo/GAZ_00041559">
        <obo:RO_0001025 rdf:resource="http://purl.obolibrary.org/obo/GAZ_00000007"/>
        <obo:IAO_0000115>An endorheic alkaline lake in Ethiopia south of Addis Ababa, in the Abijatta-Shalla National Park.</obo:IAO_0000115>
        <oboInOwl:hasOBONamespace>GAZ</oboInOwl:hasOBONamespace>
        <oboInOwl:id>GAZ:00041559</oboInOwl:id>
        <rdfs:label>Lake Abijatta</rdfs:label>
    </owl:NamedIndividual>
    


    <!-- http://purl.obolibrary.org/obo/GAZ_00041560 -->

    <owl:NamedIndividual rdf:about="http://purl.obolibrary.org/obo/GAZ_00041560">
        <obo:RO_0001025 rdf:resource="http://purl.obolibrary.org/obo/GAZ_00000007"/>
        <obo:IAO_0000115>A lake in the Southern Nations, Nationalities, and Peoples Region of Ethiopia. Located in the Great Rift Valley, east of the Guge Mountains. It is fed on its northern shore by the Bilate River, which rises on the southern slopes of Mount Gurage.</obo:IAO_0000115>
        <oboInOwl:hasOBONamespace>GAZ</oboInOwl:hasOBONamespace>
        <oboInOwl:id>GAZ:00041560</oboInOwl:id>
        <rdfs:label>Lake Abaya</rdfs:label>
    </owl:NamedIndividual>
    


    <!-- http://purl.obolibrary.org/obo/GAZ_00041561 -->

    <owl:NamedIndividual rdf:about="http://purl.obolibrary.org/obo/GAZ_00041561">
        <obo:RO_0001025 rdf:resource="http://purl.obolibrary.org/obo/GAZ_00041560"/>
        <oboInOwl:hasOBONamespace>GAZ</oboInOwl:hasOBONamespace>
        <oboInOwl:id>GAZ:00041561</oboInOwl:id>
        <rdfs:label>Aruro Island</rdfs:label>
    </owl:NamedIndividual>
    


    <!-- http://purl.obolibrary.org/obo/GAZ_00041562 -->

    <owl:NamedIndividual rdf:about="http://purl.obolibrary.org/obo/GAZ_00041562">
        <obo:RO_0001025 rdf:resource="http://purl.obolibrary.org/obo/GAZ_00041555"/>
        <obo:IAO_0000115>An island of Lake Zway.</obo:IAO_0000115>
        <oboInOwl:hasOBONamespace>GAZ</oboInOwl:hasOBONamespace>
        <oboInOwl:id>GAZ:00041562</oboInOwl:id>
        <rdfs:label>Galila Island</rdfs:label>
    </owl:NamedIndividual>
    


    <!-- http://purl.obolibrary.org/obo/GAZ_00041563 -->

    <owl:NamedIndividual rdf:about="http://purl.obolibrary.org/obo/GAZ_00041563">
        <obo:RO_0001025 rdf:resource="http://purl.obolibrary.org/obo/GAZ_00015362"/>
        <obo:RO_0001025 rdf:resource="http://purl.obolibrary.org/obo/GAZ_00015452"/>
        <obo:IAO_0000115>An island in Lake Victoria.</obo:IAO_0000115>
        <oboInOwl:hasOBONamespace>GAZ</oboInOwl:hasOBONamespace>
        <oboInOwl:id>GAZ:00041563</oboInOwl:id>
        <rdfs:label>Lolui Island</rdfs:label>
    </owl:NamedIndividual>
    


    <!-- http://purl.obolibrary.org/obo/GAZ_00041564 -->

    <owl:NamedIndividual rdf:about="http://purl.obolibrary.org/obo/GAZ_00041564">
        <obo:RO_0001025 rdf:resource="http://purl.obolibrary.org/obo/GAZ_00041555"/>
        <obo:IAO_0000115>An island of Lake Zway.</obo:IAO_0000115>
        <oboInOwl:hasOBONamespace>GAZ</oboInOwl:hasOBONamespace>
        <oboInOwl:id>GAZ:00041564</oboInOwl:id>
        <rdfs:label>Tullu Gudo Island</rdfs:label>
    </owl:NamedIndividual>
    


    <!-- http://purl.obolibrary.org/obo/GAZ_00041565 -->

    <owl:NamedIndividual rdf:about="http://purl.obolibrary.org/obo/GAZ_00041565">
        <obo:RO_0001025 rdf:resource="http://purl.obolibrary.org/obo/GAZ_00041555"/>
        <obo:IAO_0000115>An island of Lake Zway.</obo:IAO_0000115>
        <oboInOwl:hasOBONamespace>GAZ</oboInOwl:hasOBONamespace>
        <oboInOwl:id>GAZ:00041565</oboInOwl:id>
        <rdfs:label>Bird Island</rdfs:label>
    </owl:NamedIndividual>
    


    <!-- http://purl.obolibrary.org/obo/GAZ_00041566 -->

    <owl:NamedIndividual rdf:about="http://purl.obolibrary.org/obo/GAZ_00041566">
        <obo:RO_0001025 rdf:resource="http://purl.obolibrary.org/obo/GAZ_00041555"/>
        <obo:IAO_0000115>An island of Lake Zway.</obo:IAO_0000115>
        <oboInOwl:hasOBONamespace>GAZ</oboInOwl:hasOBONamespace>
        <oboInOwl:id>GAZ:00041566</oboInOwl:id>
        <rdfs:label>Debre Sina Island</rdfs:label>
    </owl:NamedIndividual>
    


    <!-- http://purl.obolibrary.org/obo/GAZ_00041571 -->

    <owl:NamedIndividual rdf:about="http://purl.obolibrary.org/obo/GAZ_00041571">
        <obo:RO_0001025 rdf:resource="http://purl.obolibrary.org/obo/GAZ_00015452"/>
        <obo:IAO_0000115>An island in Lake Victoria.</obo:IAO_0000115>
        <oboInOwl:hasOBONamespace>GAZ</oboInOwl:hasOBONamespace>
        <oboInOwl:id>GAZ:00041571</oboInOwl:id>
        <rdfs:label>Iroba Island</rdfs:label>
    </owl:NamedIndividual>
    


    <!-- http://purl.obolibrary.org/obo/GAZ_00041572 -->

    <owl:NamedIndividual rdf:about="http://purl.obolibrary.org/obo/GAZ_00041572">
        <obo:RO_0001025 rdf:resource="http://purl.obolibrary.org/obo/GAZ_00052895"/>
        <obo:IAO_0000115>An island that lies in the eastern part of Lake Victoria, at the mouth of the Winam Gulf. Part of Kenya, it lies west of Rusinga Island.</obo:IAO_0000115>
        <oboInOwl:hasOBONamespace>GAZ</oboInOwl:hasOBONamespace>
        <oboInOwl:id>GAZ:00041572</oboInOwl:id>
        <rdfs:label>Mfangano Island</rdfs:label>
    </owl:NamedIndividual>
    


    <!-- http://purl.obolibrary.org/obo/GAZ_00041573 -->

    <owl:NamedIndividual rdf:about="http://purl.obolibrary.org/obo/GAZ_00041573">
        <obo:RO_0001025 rdf:resource="http://purl.obolibrary.org/obo/GAZ_00015452"/>
        <obo:IAO_0000115>An island in Lake Victoria.</obo:IAO_0000115>
        <oboInOwl:hasOBONamespace>GAZ</oboInOwl:hasOBONamespace>
        <oboInOwl:id>GAZ:00041573</oboInOwl:id>
        <rdfs:label>Ukara Island</rdfs:label>
    </owl:NamedIndividual>
    


    <!-- http://purl.obolibrary.org/obo/GAZ_00041574 -->

    <owl:NamedIndividual rdf:about="http://purl.obolibrary.org/obo/GAZ_00041574">
        <obo:RO_0001025 rdf:resource="http://purl.obolibrary.org/obo/GAZ_00015452"/>
        <obo:IAO_0000115>An island in Lake Victoria.</obo:IAO_0000115>
        <oboInOwl:hasOBONamespace>GAZ</oboInOwl:hasOBONamespace>
        <oboInOwl:id>GAZ:00041574</oboInOwl:id>
        <rdfs:label>Kome Island [South]</rdfs:label>
    </owl:NamedIndividual>
    


    <!-- http://purl.obolibrary.org/obo/GAZ_00041575 -->

    <owl:NamedIndividual rdf:about="http://purl.obolibrary.org/obo/GAZ_00041575">
        <obo:RO_0001025 rdf:resource="http://purl.obolibrary.org/obo/GAZ_00015452"/>
        <obo:IAO_0000115>A small island in Lake Victoria, Tanzania.</obo:IAO_0000115>
        <oboInOwl:hasOBONamespace>GAZ</oboInOwl:hasOBONamespace>
        <oboInOwl:id>GAZ:00041575</oboInOwl:id>
        <rdfs:label>Nabuyongo Island</rdfs:label>
    </owl:NamedIndividual>
    


    <!-- http://purl.obolibrary.org/obo/GAZ_00041576 -->

    <owl:NamedIndividual rdf:about="http://purl.obolibrary.org/obo/GAZ_00041576">
        <obo:RO_0001025 rdf:resource="http://purl.obolibrary.org/obo/GAZ_00015452"/>
        <obo:IAO_0000115>An island in Lake Victoria.</obo:IAO_0000115>
        <oboInOwl:hasOBONamespace>GAZ</oboInOwl:hasOBONamespace>
        <oboInOwl:id>GAZ:00041576</oboInOwl:id>
        <rdfs:label>Bumbire Island</rdfs:label>
    </owl:NamedIndividual>
    


    <!-- http://purl.obolibrary.org/obo/GAZ_00041577 -->

    <owl:NamedIndividual rdf:about="http://purl.obolibrary.org/obo/GAZ_00041577">
        <obo:RO_0001025 rdf:resource="http://purl.obolibrary.org/obo/GAZ_00015452"/>
        <obo:RO_0001025 rdf:resource="http://purl.obolibrary.org/obo/GAZ_00236521"/>
        <obo:IAO_0000115>An island in Lake Victoria.</obo:IAO_0000115>
        <oboInOwl:hasOBONamespace>GAZ</oboInOwl:hasOBONamespace>
        <oboInOwl:id>GAZ:00041577</oboInOwl:id>
        <rdfs:label>Kome Island [North]</rdfs:label>
    </owl:NamedIndividual>
    


    <!-- http://purl.obolibrary.org/obo/GAZ_00041578 -->

    <owl:NamedIndividual rdf:about="http://purl.obolibrary.org/obo/GAZ_00041578">
        <obo:RO_0001025 rdf:resource="http://purl.obolibrary.org/obo/GAZ_00015452"/>
        <obo:IAO_0000115>An island in Lake Victoria.</obo:IAO_0000115>
        <oboInOwl:hasOBONamespace>GAZ</oboInOwl:hasOBONamespace>
        <oboInOwl:id>GAZ:00041578</oboInOwl:id>
        <rdfs:label>Ikuza Island</rdfs:label>
    </owl:NamedIndividual>
    


    <!-- http://purl.obolibrary.org/obo/GAZ_00041579 -->

    <owl:NamedIndividual rdf:about="http://purl.obolibrary.org/obo/GAZ_00041579">
        <obo:RO_0001025 rdf:resource="http://purl.obolibrary.org/obo/GAZ_00015452"/>
        <obo:IAO_0000115>An island that lies in the eastern part of Lake Victoria at the mouth of the Winam Gulf. Part of Kenya, it is linked to Mbita Point on the mainland by a causeway.</obo:IAO_0000115>
        <oboInOwl:hasOBONamespace>GAZ</oboInOwl:hasOBONamespace>
        <oboInOwl:id>GAZ:00041579</oboInOwl:id>
        <rdfs:label>Rusinga Island</rdfs:label>
    </owl:NamedIndividual>
    


    <!-- http://purl.obolibrary.org/obo/GAZ_00041580 -->

    <owl:NamedIndividual rdf:about="http://purl.obolibrary.org/obo/GAZ_00041580">
        <obo:RO_0001025 rdf:resource="http://purl.obolibrary.org/obo/GAZ_00052895"/>
        <obo:IAO_0000115>A small island (4.2 km2) in Winam Gulf of Lake Victoria in Kenya.</obo:IAO_0000115>
        <oboInOwl:hasOBONamespace>GAZ</oboInOwl:hasOBONamespace>
        <oboInOwl:id>GAZ:00041580</oboInOwl:id>
        <rdfs:label>Ndere Island</rdfs:label>
    </owl:NamedIndividual>
    


    <!-- http://purl.obolibrary.org/obo/GAZ_00041581 -->

    <owl:NamedIndividual rdf:about="http://purl.obolibrary.org/obo/GAZ_00041581">
        <obo:RO_0001025 rdf:resource="http://purl.obolibrary.org/obo/GAZ_00015452"/>
        <obo:IAO_0000115>An island in Lake Victoria.</obo:IAO_0000115>
        <oboInOwl:hasOBONamespace>GAZ</oboInOwl:hasOBONamespace>
        <oboInOwl:id>GAZ:00041581</oboInOwl:id>
        <rdfs:label>Bukasa Island</rdfs:label>
    </owl:NamedIndividual>
    


    <!-- http://purl.obolibrary.org/obo/GAZ_00041582 -->

    <owl:NamedIndividual rdf:about="http://purl.obolibrary.org/obo/GAZ_00041582">
        <obo:RO_0001025 rdf:resource="http://purl.obolibrary.org/obo/GAZ_00005377"/>
        <obo:RO_0001025 rdf:resource="http://purl.obolibrary.org/obo/GAZ_00015452"/>
        <obo:IAO_0000115>A small island in northern Lake Victoria. It is about 10 km south of Kampala, Uganda.</obo:IAO_0000115>
        <oboInOwl:hasOBONamespace>GAZ</oboInOwl:hasOBONamespace>
        <oboInOwl:id>GAZ:00041582</oboInOwl:id>
        <rdfs:label>Bulingugwe Island</rdfs:label>
    </owl:NamedIndividual>
    


    <!-- http://purl.obolibrary.org/obo/GAZ_00044906 -->

    <owl:NamedIndividual rdf:about="http://purl.obolibrary.org/obo/GAZ_00044906">
        <obo:RO_0001025 rdf:resource="http://purl.obolibrary.org/obo/GAZ_00000007"/>
        <obo:IAO_0000115>A fertile valley in east Lebanon. Located about 30 km east of Beirut. The valley is situated between the Mount Lebanon to the west and the Anti-Lebanon mountain ranges to the east. It forms the northeasternmost extension of the Great Rift Valley, which stretches from Syria through the Red Sea into Africa. Beqaa Valley is about 120 km in length and has an average width of about 16 km.</obo:IAO_0000115>
        <oboInOwl:hasOBONamespace>GAZ</oboInOwl:hasOBONamespace>
        <oboInOwl:id>GAZ:00044906</oboInOwl:id>
        <rdfs:label>Beqaa Valley</rdfs:label>
    </owl:NamedIndividual>
    


    <!-- http://purl.obolibrary.org/obo/GAZ_00044911 -->

    <owl:NamedIndividual rdf:about="http://purl.obolibrary.org/obo/GAZ_00044911">
        <obo:RO_0001025 rdf:resource="http://purl.obolibrary.org/obo/GAZ_00248126"/>
        <obo:IAO_0000115>An endorheic saline lake in Southern Ethiopia on the boundary between the Oromia and the Southern Nations, Nationalities and Peoples&apos; Regions. When the lake is filled, it stretches into northern Kenya. Lying at the center of the Stephanie Wildlife Reserve, the lake measures some 40 miles by 15 miles. This lake is the southernmost and lowest (1,880 feet) of a series of lakes which lie in the north-easterly continuation of the Great Rift Valley; its watershed is separated from the watershed of Lake Turkana by the Humu Range and the hills south of it. The Kumbi Range rises on its eastern side. Chew Bahir is fed from the north by the Weito River, and its tributary the Galana Sagan. The Galana Sagan receives the overflow of Lake Chamo in some years, but no permanent connection exists.</obo:IAO_0000115>
        <oboInOwl:hasOBONamespace>GAZ</oboInOwl:hasOBONamespace>
        <oboInOwl:id>GAZ:00044911</oboInOwl:id>
        <rdfs:label>Lake Bahir</rdfs:label>
    </owl:NamedIndividual>
    


    <!-- http://purl.obolibrary.org/obo/GAZ_00044914 -->

    <owl:NamedIndividual rdf:about="http://purl.obolibrary.org/obo/GAZ_00044914">
        <obo:RO_0001025 rdf:resource="http://purl.obolibrary.org/obo/GAZ_00007520"/>
        <obo:IAO_0000115>A freshwater monomictic lake, being approximately 53 km in circumference, about 21 km long, and 13 km wide. The lake has a total area of 166 km2, and a maximum depth of approximately 43 m. It is situated deep in the Jordan Great Rift Valley, the valley caused by the separation of the African and Arabian Plates and is fed partly by underground springs although its main source is the Jordan River which flows through it from north to south. Consequently the area is subject to earthquakes and, in the past, volcanic activity. This is evidenced by the abundant basalt and other igneous rocks that define the geology of the Galilee region.</obo:IAO_0000115>
        <oboInOwl:hasOBONamespace>GAZ</oboInOwl:hasOBONamespace>
        <oboInOwl:id>GAZ:00044914</oboInOwl:id>
        <rdfs:label>Sea of Galilee</rdfs:label>
    </owl:NamedIndividual>
    


    <!-- http://purl.obolibrary.org/obo/GAZ_00044915 -->

    <owl:NamedIndividual rdf:about="http://purl.obolibrary.org/obo/GAZ_00044915">
        <obo:RO_0001025 rdf:resource="http://purl.obolibrary.org/obo/GAZ_00000007"/>
        <obo:IAO_0000115>A 375 km long strike-slip fault zone some 5 km wide in the north and 23 km wide in the south that forms part of the broader Great Rift Valley. Located in modern-day Israel, Jordan, the West Bank and the Golan Heights, this geographic region includes the Jordan River, Hula Valley, Lake Tiberias and the Dead Sea, features created by the physiographic and geologic process underway.</obo:IAO_0000115>
        <oboInOwl:hasOBONamespace>GAZ</oboInOwl:hasOBONamespace>
        <oboInOwl:id>GAZ:00044915</oboInOwl:id>
        <rdfs:label>Jordan Rift Valley</rdfs:label>
    </owl:NamedIndividual>
    


    <!-- http://purl.obolibrary.org/obo/GAZ_00044916 -->

    <owl:NamedIndividual rdf:about="http://purl.obolibrary.org/obo/GAZ_00044916">
        <obo:RO_0001025 rdf:resource="http://purl.obolibrary.org/obo/GAZ_00000007"/>
        <obo:RO_0001025 rdf:resource="http://purl.obolibrary.org/obo/GAZ_00044915"/>
        <obo:IAO_0000115>A section of the Great Rift Valley lying between the Dead Sea to the north and the Gulf of Aqaba or the Gulf of Eilat to the south. It forms part of the border between Israel to the west and Jordan to the east.</obo:IAO_0000115>
        <oboInOwl:hasOBONamespace>GAZ</oboInOwl:hasOBONamespace>
        <oboInOwl:id>GAZ:00044916</oboInOwl:id>
        <rdfs:label>Wadi Arabah</rdfs:label>
    </owl:NamedIndividual>
    


    <!-- http://purl.obolibrary.org/obo/GAZ_00049007 -->

    <owl:NamedIndividual rdf:about="http://purl.obolibrary.org/obo/GAZ_00049007">
        <obo:RO_0001025 rdf:resource="http://purl.obolibrary.org/obo/GAZ_00007862"/>
        <obo:IAO_0000115>The narrow sea passages, about 13 km wide, between the Sinai and Arabian peninsulas which separates the Gulf of Aqaba from the Red Sea.</obo:IAO_0000115>
        <oboInOwl:hasOBONamespace>GAZ</oboInOwl:hasOBONamespace>
        <oboInOwl:id>GAZ:00049007</oboInOwl:id>
        <rdfs:label>Straits of Tiran</rdfs:label>
    </owl:NamedIndividual>
    


    <!-- http://purl.obolibrary.org/obo/GAZ_00049008 -->

    <owl:NamedIndividual rdf:about="http://purl.obolibrary.org/obo/GAZ_00049008">
        <obo:RO_0001025 rdf:resource="http://purl.obolibrary.org/obo/GAZ_00049007"/>
        <obo:IAO_0000115>A Saudi Arabian island in the Straits of Tiran east of Tiran Island.</obo:IAO_0000115>
        <oboInOwl:hasOBONamespace>GAZ</oboInOwl:hasOBONamespace>
        <oboInOwl:id>GAZ:00049008</oboInOwl:id>
        <rdfs:label>Sanafir Island</rdfs:label>
    </owl:NamedIndividual>
    


    <!-- http://purl.obolibrary.org/obo/GAZ_00049009 -->

    <owl:NamedIndividual rdf:about="http://purl.obolibrary.org/obo/GAZ_00049009">
        <obo:RO_0001025 rdf:resource="http://purl.obolibrary.org/obo/GAZ_00049007"/>
        <obo:IAO_0000115>An island belonging to Saudi Arabia at the entrance of the Straits of Tiran, which separates the Red Sea and the Gulf of Aqaba.</obo:IAO_0000115>
        <oboInOwl:hasOBONamespace>GAZ</oboInOwl:hasOBONamespace>
        <oboInOwl:id>GAZ:00049009</oboInOwl:id>
        <rdfs:label>Tiran Island</rdfs:label>
    </owl:NamedIndividual>
    


    <!-- http://purl.obolibrary.org/obo/GAZ_00051205 -->

    <owl:NamedIndividual rdf:about="http://purl.obolibrary.org/obo/GAZ_00051205">
        <obo:RO_0001025 rdf:resource="http://purl.obolibrary.org/obo/GAZ_00000007"/>
        <obo:IAO_0000115>A geological depression in the Horn of Africa, where it overlaps Eritrea, the Afar Region of Ethiopia, and Djibouti. Only the Awash River flows into the depression, where it ends in a chain of lakes that increase in salinity.</obo:IAO_0000115>
        <oboInOwl:hasOBONamespace>GAZ</oboInOwl:hasOBONamespace>
        <oboInOwl:id>GAZ:00051205</oboInOwl:id>
        <rdfs:label>Afar Depression</rdfs:label>
    </owl:NamedIndividual>
    


    <!-- http://purl.obolibrary.org/obo/GAZ_00052567 -->

    <owl:NamedIndividual rdf:about="http://purl.obolibrary.org/obo/GAZ_00052567">
        <obo:IAO_0000115>A river of southern Ethiopia. Its course is entirely contained within the boundaries of Ethiopia, and empties into Lake Turkana on the border with Kenya. It is the principal stream of an endorheic drainage basin; the part that the Omo drains includes part of the western Oromia Region and the middle of the Southern Nations, Nationalities, and People&apos;s Region. This river rises in the Shewan highlands and is a perennial river. Its course is generally to the south, however with a major bend to the west at about 7deg N 37deg 30minE to about 36deg E where it turns south until 5deg 30min N where it makes a large S- bend then resumes its southernly course to Lake Turkana.</obo:IAO_0000115>
        <oboInOwl:hasOBONamespace>GAZ</oboInOwl:hasOBONamespace>
        <oboInOwl:id>GAZ:00052567</oboInOwl:id>
        <rdfs:label>Omo River</rdfs:label>
    </owl:NamedIndividual>
    


    <!-- http://purl.obolibrary.org/obo/GAZ_00052683 -->

    <owl:NamedIndividual rdf:about="http://purl.obolibrary.org/obo/GAZ_00052683">
        <obo:RO_0001025 rdf:resource="http://purl.obolibrary.org/obo/GAZ_00051205"/>
        <obo:IAO_0000115>A saline lake in the northern end of the Afar Depression, Ethiopia.</obo:IAO_0000115>
        <oboInOwl:hasOBONamespace>GAZ</oboInOwl:hasOBONamespace>
        <oboInOwl:id>GAZ:00052683</oboInOwl:id>
        <rdfs:label>Lake Karum</rdfs:label>
    </owl:NamedIndividual>
    


    <!-- http://purl.obolibrary.org/obo/GAZ_00052684 -->

    <owl:NamedIndividual rdf:about="http://purl.obolibrary.org/obo/GAZ_00052684">
        <obo:RO_0001025 rdf:resource="http://purl.obolibrary.org/obo/GAZ_00051205"/>
        <obo:IAO_0000115>A saline crater lake in central Djibouti, located at the southern border of Tadjoura Region, touching Dikhil Region. Fed by subterranean inflows which include infiltration of sea water, as well as by wadis which lead into the depression.</obo:IAO_0000115>
        <oboInOwl:hasOBONamespace>GAZ</oboInOwl:hasOBONamespace>
        <oboInOwl:id>GAZ:00052684</oboInOwl:id>
        <rdfs:label>Lake Asal</rdfs:label>
    </owl:NamedIndividual>
    


    <!-- http://purl.obolibrary.org/obo/GAZ_00052883 -->

    <owl:NamedIndividual rdf:about="http://purl.obolibrary.org/obo/GAZ_00052883">
        <obo:IAO_0000115>A dam on the Yarmuk River.</obo:IAO_0000115>
        <oboInOwl:hasOBONamespace>GAZ</oboInOwl:hasOBONamespace>
        <oboInOwl:id>GAZ:00052883</oboInOwl:id>
        <rdfs:label>Maqarin Dam</rdfs:label>
    </owl:NamedIndividual>
    


    <!-- http://purl.obolibrary.org/obo/GAZ_00052895 -->

    <owl:NamedIndividual rdf:about="http://purl.obolibrary.org/obo/GAZ_00052895">
        <obo:RO_0001025 rdf:resource="http://purl.obolibrary.org/obo/GAZ_00015452"/>
        <obo:IAO_0000115>A significant extension of northeastern Lake Victoria into western Kenya. It is a shallow inlet and is connected to the main lake by Rusinga Channel (3 mi wide), which is partly masked from the main body of the lake by islands. The port of Kisumu, Kenya&apos;s fourth largest city, stands on its northeastern shore.</obo:IAO_0000115>
        <oboInOwl:hasOBONamespace>GAZ</oboInOwl:hasOBONamespace>
        <oboInOwl:id>GAZ:00052895</oboInOwl:id>
        <rdfs:label>Winam Gulf</rdfs:label>
    </owl:NamedIndividual>
    


    <!-- http://purl.obolibrary.org/obo/GAZ_00052896 -->

    <owl:NamedIndividual rdf:about="http://purl.obolibrary.org/obo/GAZ_00052896">
        <obo:RO_0001025 rdf:resource="http://purl.obolibrary.org/obo/GAZ_00052895"/>
        <oboInOwl:hasOBONamespace>GAZ</oboInOwl:hasOBONamespace>
        <oboInOwl:id>GAZ:00052896</oboInOwl:id>
        <rdfs:label>Asembo Bay</rdfs:label>
    </owl:NamedIndividual>
    


    <!-- http://purl.obolibrary.org/obo/GAZ_00052899 -->

    <owl:NamedIndividual rdf:about="http://purl.obolibrary.org/obo/GAZ_00052899">
        <obo:RO_0001025 rdf:resource="http://purl.obolibrary.org/obo/GAZ_00007523"/>
        <oboInOwl:hasOBONamespace>GAZ</oboInOwl:hasOBONamespace>
        <oboInOwl:id>GAZ:00052899</oboInOwl:id>
        <rdfs:label>Causeway Pond</rdfs:label>
    </owl:NamedIndividual>
    


    <!-- http://purl.obolibrary.org/obo/GAZ_00052911 -->

    <owl:NamedIndividual rdf:about="http://purl.obolibrary.org/obo/GAZ_00052911">
        <obo:RO_0001025 rdf:resource="http://purl.obolibrary.org/obo/GAZ_00052895"/>
        <obo:IAO_0000115>A bay on the south shore of Winam Gulf of Lake Victoria, in western Kenya.</obo:IAO_0000115>
        <oboInOwl:hasOBONamespace>GAZ</oboInOwl:hasOBONamespace>
        <oboInOwl:id>GAZ:00052911</oboInOwl:id>
        <rdfs:label>Homa Bay</rdfs:label>
    </owl:NamedIndividual>
    


    <!-- http://purl.obolibrary.org/obo/GAZ_00052985 -->

    <owl:NamedIndividual rdf:about="http://purl.obolibrary.org/obo/GAZ_00052985">
        <obo:RO_0001025 rdf:resource="http://purl.obolibrary.org/obo/GAZ_00000007"/>
        <oboInOwl:hasOBONamespace>GAZ</oboInOwl:hasOBONamespace>
        <oboInOwl:id>GAZ:00052985</oboInOwl:id>
        <rdfs:label>Laikipia Plateau</rdfs:label>
    </owl:NamedIndividual>
    


    <!-- http://purl.obolibrary.org/obo/GAZ_00052986 -->

    <owl:NamedIndividual rdf:about="http://purl.obolibrary.org/obo/GAZ_00052986">
        <obo:RO_0001025 rdf:resource="http://purl.obolibrary.org/obo/GAZ_00052985"/>
        <obo:IAO_0000115>A research center.</obo:IAO_0000115>
        <oboInOwl:hasOBONamespace>GAZ</oboInOwl:hasOBONamespace>
        <oboInOwl:id>GAZ:00052986</oboInOwl:id>
        <rdfs:label>Mpala Research Centre</rdfs:label>
    </owl:NamedIndividual>
    


    <!-- http://purl.obolibrary.org/obo/GAZ_00053520 -->

    <owl:NamedIndividual rdf:about="http://purl.obolibrary.org/obo/GAZ_00053520">
        <obo:RO_0001025 rdf:resource="http://purl.obolibrary.org/obo/GAZ_00015396"/>
        <obo:IAO_0000115>A volcanic field of carbonatite lavas and tuffs of the Fort Portal volcanic field in Uganda, NE of Mount Ruwenzori between Lake Albert and Lake Edward. It consists of a group of tuff cones and maars. About 50 volcanic vents, some of which now contain crater lakes, were erupted through basement rocks of Precambrian gneiss in an WSW-ENE-trending area north of the town of Fort Portal.</obo:IAO_0000115>
        <oboInOwl:hasOBONamespace>GAZ</oboInOwl:hasOBONamespace>
        <oboInOwl:id>GAZ:00053520</oboInOwl:id>
        <rdfs:label>Fort Portal Volcanic Field</rdfs:label>
    </owl:NamedIndividual>
    


    <!-- http://purl.obolibrary.org/obo/GAZ_00053521 -->

    <owl:NamedIndividual rdf:about="http://purl.obolibrary.org/obo/GAZ_00053521">
        <obo:RO_0001025 rdf:resource="http://purl.obolibrary.org/obo/GAZ_00015396"/>
        <obo:IAO_0000115>A volcanic field that occupies the Western Rift Valley, east of the Ruwenzori Mountains halfway between Lake Edward and Lake Albert. The Kyatwa tuff cones and lake-filled maars are part of a group of Pleistocene-to-Recent volcanic fields in western Uganda.</obo:IAO_0000115>
        <oboInOwl:hasOBONamespace>GAZ</oboInOwl:hasOBONamespace>
        <oboInOwl:id>GAZ:00053521</oboInOwl:id>
        <rdfs:label>Kyatwa Volcanic Field</rdfs:label>
    </owl:NamedIndividual>
    


    <!-- http://purl.obolibrary.org/obo/GAZ_00053522 -->

    <owl:NamedIndividual rdf:about="http://purl.obolibrary.org/obo/GAZ_00053522">
        <obo:RO_0001025 rdf:resource="http://purl.obolibrary.org/obo/GAZ_00015394"/>
        <obo:RO_0001025 rdf:resource="http://purl.obolibrary.org/obo/GAZ_00076731"/>
        <obo:IAO_0000115>A volcanic field, stretching from the NE shore of Lake Edward to the western shore of Lake George. It is the most extensive of a series of volcanic fields in the Western Rift Valley of Uganda. The volcanic field contains a group of foiditic tuff cones and maars, some of which are filled by lakes. Lake Katwe is a shallow 3 km-long body of water that occupies two of three intersecting craters immediately NE of Lake Edward.</obo:IAO_0000115>
        <oboInOwl:hasOBONamespace>GAZ</oboInOwl:hasOBONamespace>
        <oboInOwl:id>GAZ:00053522</oboInOwl:id>
        <rdfs:label>Katwe-Kikorongo Volcanic Field</rdfs:label>
    </owl:NamedIndividual>
    


    <!-- http://purl.obolibrary.org/obo/GAZ_00053523 -->

    <owl:NamedIndividual rdf:about="http://purl.obolibrary.org/obo/GAZ_00053523">
        <obo:RO_0001025 rdf:resource="http://purl.obolibrary.org/obo/GAZ_00053522"/>
        <obo:RO_0001025 rdf:resource="http://purl.obolibrary.org/obo/GAZ_00076731"/>
        <obo:IAO_0000115>A crater lake that occupies two of three intersecting craters immediately NE of Lake Edward.</obo:IAO_0000115>
        <oboInOwl:hasOBONamespace>GAZ</oboInOwl:hasOBONamespace>
        <oboInOwl:id>GAZ:00053523</oboInOwl:id>
        <rdfs:label>Lake Katwe</rdfs:label>
    </owl:NamedIndividual>
    


    <!-- http://purl.obolibrary.org/obo/GAZ_00053524 -->

    <owl:NamedIndividual rdf:about="http://purl.obolibrary.org/obo/GAZ_00053524">
        <obo:RO_0001025 rdf:resource="http://purl.obolibrary.org/obo/GAZ_00076731"/>
        <obo:IAO_0000115>A volcanic field that lies along the eastern side of the Western Rift Valley, south of Lake George. It contains more than 130 maars, 27 of which contain lakes with water ranging from fresh to saline. Friable calcareous volcanic tuffs are inter-bedded with Pleistocene and Recent sediments. Only a few foiditic lava flows are found in the volcanic field.</obo:IAO_0000115>
        <oboInOwl:hasOBONamespace>GAZ</oboInOwl:hasOBONamespace>
        <oboInOwl:id>GAZ:00053524</oboInOwl:id>
        <rdfs:label>Bunyaruguru Volcanic Field</rdfs:label>
    </owl:NamedIndividual>
    


    <!-- http://purl.obolibrary.org/obo/GAZ_00053525 -->

    <owl:NamedIndividual rdf:about="http://purl.obolibrary.org/obo/GAZ_00053525">
        <obo:RO_0001025 rdf:resource="http://purl.obolibrary.org/obo/GAZ_00015405"/>
        <obo:IAO_0000115>An isolated tuff cone with associated lava flows located east of Lake Edward, is the southernmost feature of a N-S-trending chain of high-potassium foditic volcanic fields in the Western Rift Valley of Uganda. Katunga is the type locality of the rock type katungite, an olivine-melilitite.</obo:IAO_0000115>
        <oboInOwl:hasOBONamespace>GAZ</oboInOwl:hasOBONamespace>
        <oboInOwl:id>GAZ:00053525</oboInOwl:id>
        <rdfs:label>Katunga</rdfs:label>
    </owl:NamedIndividual>
    


    <!-- http://purl.obolibrary.org/obo/GAZ_00053526 -->

    <owl:NamedIndividual rdf:about="http://purl.obolibrary.org/obo/GAZ_00053526">
        <obo:RO_0001025 rdf:resource="http://purl.obolibrary.org/obo/GAZ_00053536"/>
        <obo:IAO_0000115>An extinct stratovolcano in the Virunga Mountains on the border between Rwanda and Uganda. At 4,127 m, Muhabura is the third highest of the eight major mountains of the mountain range, which is a part of the East African Rift Valley. Muhabura lies partly in Volcanoes National Park, Rwanda and partly in Mgahinga Gorilla National Park, Uganda.</obo:IAO_0000115>
        <oboInOwl:hasOBONamespace>GAZ</oboInOwl:hasOBONamespace>
        <oboInOwl:id>GAZ:00053526</oboInOwl:id>
        <rdfs:label>Mount Muhabura</rdfs:label>
    </owl:NamedIndividual>
    


    <!-- http://purl.obolibrary.org/obo/GAZ_00053528 -->

    <owl:NamedIndividual rdf:about="http://purl.obolibrary.org/obo/GAZ_00053528">
        <obo:IAO_0000115>A stratovolcano in the Virunga Mountains associated with the Great Rift Valley. It is located in the Democratic Republic of the Congo, about 20 km north of the town of Goma and Lake Kivu and just west of the border with Rwanda. It contained a lava lake in its deep summit crater that was active for half a century before draining catastrophically through its outer flanks in 1977. In contrast to the low profile of its neighboring shield volcano, Nyamuragira, 3470 m high Nyiragongo displays the steep slopes of a stratovolcano. Benches in the steep-walled, 1.2 km wide summit crater mark levels of former lava lakes, which have been observed since the late-19th century. Two older stratovolcanoes, Baruta and Shaheru, are partially overlapped by Nyiragongo on the north and south. About 100 parasitic cones are located primarily along radial fissures south of Shaheru, east of the summit, and along a NE-SW zone extending as far as Lake Kivu. Many cones are buried by voluminous lava flows that extend long distances down the flanks of the volcano, which is characterized by the eruption of foiditic rocks.</obo:IAO_0000115>
        <oboInOwl:hasOBONamespace>GAZ</oboInOwl:hasOBONamespace>
        <oboInOwl:id>GAZ:00053528</oboInOwl:id>
        <rdfs:label>Mount Nyiragongo</rdfs:label>
    </owl:NamedIndividual>
    


    <!-- http://purl.obolibrary.org/obo/GAZ_00053529 -->

    <owl:NamedIndividual rdf:about="http://purl.obolibrary.org/obo/GAZ_00053529">
        <obo:IAO_0000115>An active volcano in the Virunga Mountains of the Democratic Republic of the Congo, situated about 25 km north of Lake Kivu. A massive high-potassium basaltic shield volcano that rises about 25 km north of Lake Kivu across the broad East African Rift Valley NW of Nyiragongo volcano. Nyamuragira, also known as Nyamulagira, has a volume of 500 cu km, and extensive lava flows from the volcano blanket 1500 km2 of the East African Rift. The broad low-angle shield volcano contrasts dramatically with its steep-sided neighbor Nyiragongo. The 3058 m high summit of Nyamuragira is truncated by a small 2 x 2.3 km caldera that has walls up to about 100 m high.</obo:IAO_0000115>
        <oboInOwl:hasOBONamespace>GAZ</oboInOwl:hasOBONamespace>
        <oboInOwl:id>GAZ:00053529</oboInOwl:id>
        <rdfs:label>Mount Nyamuragira</rdfs:label>
    </owl:NamedIndividual>
    


    <!-- http://purl.obolibrary.org/obo/GAZ_00053530 -->

    <owl:NamedIndividual rdf:about="http://purl.obolibrary.org/obo/GAZ_00053530">
        <obo:IAO_0000115>A dormant volcano in the Virunga Mountains on the border between Rwanda and the Democratic Republic of Congo. A complex stratovolcano with a symmetrical sharp-peaked summit. The 2 km wide Branca caldera, located SE of the 4507 m high summit, is filled by viscous lava flows and two explosion craters. The large, 1.2 km wide Muntango pit crater is located south of the summit of the basanitic-to-trachytic volcano. A broad lava plain, formed from lava flows erupted within the caldera and along a chain of parasitic cones, extends SW. More than 100 parasitic cones erupted along a NNE-SSW zone that extends to the shores of Lake Kivu.</obo:IAO_0000115>
        <oboInOwl:hasOBONamespace>GAZ</oboInOwl:hasOBONamespace>
        <oboInOwl:id>GAZ:00053530</oboInOwl:id>
        <rdfs:label>Mount Karisimbi</rdfs:label>
    </owl:NamedIndividual>
    


    <!-- http://purl.obolibrary.org/obo/GAZ_00053533 -->

    <owl:NamedIndividual rdf:about="http://purl.obolibrary.org/obo/GAZ_00053533">
        <oboInOwl:hasOBONamespace>GAZ</oboInOwl:hasOBONamespace>
        <oboInOwl:id>GAZ:00053533</oboInOwl:id>
        <rdfs:label>Mount Mikeno</rdfs:label>
    </owl:NamedIndividual>
    


    <!-- http://purl.obolibrary.org/obo/GAZ_00053534 -->

    <owl:NamedIndividual rdf:about="http://purl.obolibrary.org/obo/GAZ_00053534">
        <obo:IAO_0000115>An extinct volcano in the Virunga Mountains of the Great Rift Valley. It straddles the border of Rwanda and the Democratic Republic of the Congo, but the summit is located in Rwanda.</obo:IAO_0000115>
        <oboInOwl:hasOBONamespace>GAZ</oboInOwl:hasOBONamespace>
        <oboInOwl:id>GAZ:00053534</oboInOwl:id>
        <rdfs:label>Mount Bisoke</rdfs:label>
    </owl:NamedIndividual>
    


    <!-- http://purl.obolibrary.org/obo/GAZ_00053535 -->

    <owl:NamedIndividual rdf:about="http://purl.obolibrary.org/obo/GAZ_00053535">
        <obo:RO_0001025 rdf:resource="http://purl.obolibrary.org/obo/GAZ_00053536"/>
        <obo:IAO_0000115>An extinct volcano in eastern Africa, in the Virunga Mountains. The summit of the mountain, at 3645 m marks the intersection of the borders of the Democratic Republic of the Congo, Rwanda, and Uganda.</obo:IAO_0000115>
        <oboInOwl:hasOBONamespace>GAZ</oboInOwl:hasOBONamespace>
        <oboInOwl:id>GAZ:00053535</oboInOwl:id>
        <rdfs:label>Mount Sabyinyo</rdfs:label>
    </owl:NamedIndividual>
    


    <!-- http://purl.obolibrary.org/obo/GAZ_00053536 -->

    <owl:NamedIndividual rdf:about="http://purl.obolibrary.org/obo/GAZ_00053536">
        <obo:RO_0001025 rdf:resource="http://purl.obolibrary.org/obo/GAZ_00015410"/>
        <obo:IAO_0000115>A national park in the far south-west of Uganda near the town of Kisoro. It is located in the Virunga Mountains and is conterminous with the Volcanoes National Park in Rwanda and the Virunga National Park in the Democratic Republic of the Congo.</obo:IAO_0000115>
        <oboInOwl:hasOBONamespace>GAZ</oboInOwl:hasOBONamespace>
        <oboInOwl:id>GAZ:00053536</oboInOwl:id>
        <rdfs:label>Mgahinga Gorilla National Park</rdfs:label>
    </owl:NamedIndividual>
    


    <!-- http://purl.obolibrary.org/obo/GAZ_00053537 -->

    <owl:NamedIndividual rdf:about="http://purl.obolibrary.org/obo/GAZ_00053537">
        <obo:RO_0001025 rdf:resource="http://purl.obolibrary.org/obo/GAZ_00053536"/>
        <obo:IAO_0000115>A dormant/extinct volcano in the Virunga Mountains on the border between Rwanda and Uganda. Gahinga lies between Muhahabura and Sabyinyo, but is the smallest of these three.</obo:IAO_0000115>
        <oboInOwl:hasOBONamespace>GAZ</oboInOwl:hasOBONamespace>
        <oboInOwl:id>GAZ:00053537</oboInOwl:id>
        <rdfs:label>Mount Gahinga</rdfs:label>
    </owl:NamedIndividual>
    


    <!-- http://purl.obolibrary.org/obo/GAZ_00053539 -->

    <owl:NamedIndividual rdf:about="http://purl.obolibrary.org/obo/GAZ_00053539">
        <obo:RO_0001025 rdf:resource="http://purl.obolibrary.org/obo/GAZ_00053530"/>
        <obo:IAO_0000115>A crater located south of the summit of the basanitic-to-trachytic Karisimbi volcano.</obo:IAO_0000115>
        <oboInOwl:hasOBONamespace>GAZ</oboInOwl:hasOBONamespace>
        <oboInOwl:id>GAZ:00053539</oboInOwl:id>
        <rdfs:label>Muntango Pit Crater</rdfs:label>
    </owl:NamedIndividual>
    


    <!-- http://purl.obolibrary.org/obo/GAZ_00053540 -->

    <owl:NamedIndividual rdf:about="http://purl.obolibrary.org/obo/GAZ_00053540">
        <obo:IAO_0000115>A stratovolcano that is the NE-most of a cluster of large stratovolcanoes at the southern end of the Virunga Range on the border of the Democratic Republic of Congo and Rwanda.</obo:IAO_0000115>
        <oboInOwl:hasOBONamespace>GAZ</oboInOwl:hasOBONamespace>
        <oboInOwl:id>GAZ:00053540</oboInOwl:id>
        <rdfs:label>Mount Visoke</rdfs:label>
    </owl:NamedIndividual>
    


    <!-- http://purl.obolibrary.org/obo/GAZ_00053541 -->

    <owl:NamedIndividual rdf:about="http://purl.obolibrary.org/obo/GAZ_00053541">
        <obo:RO_0001025 rdf:resource="http://purl.obolibrary.org/obo/GAZ_00015410"/>
        <obo:IAO_0000115>A volcanic field in SW Uganda that consists of a group of about 40 cinder cones lying north of the large stratovolcanoes of the NE part of the Virunga Mountains. The cinder cones occur in clusters and were erupted along lineaments. They are typically breached on one side by lava flows.</obo:IAO_0000115>
        <oboInOwl:hasOBONamespace>GAZ</oboInOwl:hasOBONamespace>
        <oboInOwl:id>GAZ:00053541</oboInOwl:id>
        <rdfs:label>Bufumbira Volcanic Field</rdfs:label>
    </owl:NamedIndividual>
    


    <!-- http://purl.obolibrary.org/obo/GAZ_00053543 -->

    <owl:NamedIndividual rdf:about="http://purl.obolibrary.org/obo/GAZ_00053543">
        <obo:RO_0001025 rdf:resource="http://purl.obolibrary.org/obo/GAZ_00076409"/>
        <obo:IAO_0000115>A non-solutional cave developed in pyroclastic (volcanic) rocks (not, as some have presumed, a lava tube) in Mount Elgon National Park in Kenya. The cave extends about 200 m into the side of the mountain.</obo:IAO_0000115>
        <oboInOwl:hasOBONamespace>GAZ</oboInOwl:hasOBONamespace>
        <oboInOwl:id>GAZ:00053543</oboInOwl:id>
        <rdfs:label>Kitum Cave</rdfs:label>
    </owl:NamedIndividual>
    


    <!-- http://purl.obolibrary.org/obo/GAZ_00053546 -->

    <owl:NamedIndividual rdf:about="http://purl.obolibrary.org/obo/GAZ_00053546">
        <obo:RO_0001025 rdf:resource="http://purl.obolibrary.org/obo/GAZ_00000007"/>
        <obo:IAO_0000115>A volcanic complex separates Lake Turkana from the broad Suguta Trough to the south, the site of a former lake. The volcano is comprised of four overlapping shield volcanoes, with the youngest, Kakorinya, located over the axis of the East African Rift. Kalolenyang volcano lies west of Kakorinya, and Likaiu West and Likaiu East volcano are located to the ENE. A 3.8 km wide summit caldera was formed at Kakorinya volcano about 92,000 years ago. Youthful-looking trachytic and phonolitic lava domes and flows erupted within the caldera and along its ring fracture fill much of the caldera floor. Early Holocene fissure-related scoria cones and lava flows dot the volcano&apos;s southern and northern flanks. Solfataric fields are located within the caldera and on the western and southern flanks of the volcano.</obo:IAO_0000115>
        <oboInOwl:hasOBONamespace>GAZ</oboInOwl:hasOBONamespace>
        <oboInOwl:id>GAZ:00053546</oboInOwl:id>
        <rdfs:label>The Barrier Volcanic Complex</rdfs:label>
    </owl:NamedIndividual>
    


    <!-- http://purl.obolibrary.org/obo/GAZ_00053547 -->

    <owl:NamedIndividual rdf:about="http://purl.obolibrary.org/obo/GAZ_00053547">
        <obo:RO_0001025 rdf:resource="http://purl.obolibrary.org/obo/GAZ_00053546"/>
        <obo:IAO_0000115>A volcano in the Barrier Complex.</obo:IAO_0000115>
        <oboInOwl:hasOBONamespace>GAZ</oboInOwl:hasOBONamespace>
        <oboInOwl:id>GAZ:00053547</oboInOwl:id>
        <rdfs:label>Kakorinya Volcano</rdfs:label>
    </owl:NamedIndividual>
    


    <!-- http://purl.obolibrary.org/obo/GAZ_00053548 -->

    <owl:NamedIndividual rdf:about="http://purl.obolibrary.org/obo/GAZ_00053548">
        <obo:RO_0001025 rdf:resource="http://purl.obolibrary.org/obo/GAZ_00053546"/>
        <obo:IAO_0000115>A volcano in the Barrier Complex.</obo:IAO_0000115>
        <oboInOwl:hasOBONamespace>GAZ</oboInOwl:hasOBONamespace>
        <oboInOwl:id>GAZ:00053548</oboInOwl:id>
        <rdfs:label>Likaiu East Volcano</rdfs:label>
    </owl:NamedIndividual>
    


    <!-- http://purl.obolibrary.org/obo/GAZ_00053549 -->

    <owl:NamedIndividual rdf:about="http://purl.obolibrary.org/obo/GAZ_00053549">
        <obo:RO_0001025 rdf:resource="http://purl.obolibrary.org/obo/GAZ_00053546"/>
        <obo:IAO_0000115>A volcano in the Barrier Complex.</obo:IAO_0000115>
        <oboInOwl:hasOBONamespace>GAZ</oboInOwl:hasOBONamespace>
        <oboInOwl:id>GAZ:00053549</oboInOwl:id>
        <rdfs:label>Kakorinya Volcano</rdfs:label>
    </owl:NamedIndividual>
    


    <!-- http://purl.obolibrary.org/obo/GAZ_00053550 -->

    <owl:NamedIndividual rdf:about="http://purl.obolibrary.org/obo/GAZ_00053550">
        <obo:RO_0001025 rdf:resource="http://purl.obolibrary.org/obo/GAZ_00053546"/>
        <obo:IAO_0000115>A volcano in the Barrier Complex.</obo:IAO_0000115>
        <oboInOwl:hasOBONamespace>GAZ</oboInOwl:hasOBONamespace>
        <oboInOwl:id>GAZ:00053550</oboInOwl:id>
        <rdfs:label>Likaiu West Volcano</rdfs:label>
    </owl:NamedIndividual>
    


    <!-- http://purl.obolibrary.org/obo/GAZ_00053551 -->

    <owl:NamedIndividual rdf:about="http://purl.obolibrary.org/obo/GAZ_00053551">
        <obo:RO_0001025 rdf:resource="http://purl.obolibrary.org/obo/GAZ_00000007"/>
        <obo:IAO_0000115>A trachytic shield volcano is topped by parasitic cones and lava flows of upper Pleistocene and Holocene age. Voluminous basaltic effusive and explosive activity took place during the early Holocene on the lower northern, eastern, and southern flanks along the axis of the East African Rift, producing fissure-controlled subaerial basaltic scoria cones and lava flows, and partially or completely sublacustral tuff cones, tuff rings, and pillow lavas. Fluid olivine basalts were also erupted from a breached scoria cone forming the summit of Namarunu.</obo:IAO_0000115>
        <oboInOwl:hasOBONamespace>GAZ</oboInOwl:hasOBONamespace>
        <oboInOwl:id>GAZ:00053551</oboInOwl:id>
        <rdfs:label>Namarunu Volcano</rdfs:label>
    </owl:NamedIndividual>
    


    <!-- http://purl.obolibrary.org/obo/GAZ_00053554 -->

    <owl:NamedIndividual rdf:about="http://purl.obolibrary.org/obo/GAZ_00053554">
        <obo:RO_0001025 rdf:resource="http://purl.obolibrary.org/obo/GAZ_00000007"/>
        <obo:IAO_0000115>A shield volcano is situated at a narrow constriction in the Rift Valley and almost completely straddles it. A 5 x 3.5 km summit caldera formed about 38,000 years ago. Since then trachytic and basaltic lava flows were erupted on the northern and southern flanks and within the caldera. A NNE-SSW-trending chain of lake-filled basaltic maars extends along the floor of the rift from the lower flanks of the volcano. Young lava flows were also erupted from vents along rift valley faults. Well-preserved parasitic cones erupted along rift-parallel faults cutting the volcano abound; the latest eruption produced a trachytic lava flow dated from secular magnetic variation measurements at about the beginning of the 20th century. Fumarolic activity and hot steaming ground occurs along NNE-trending fissures within the caldera and along the lower NW flanks.</obo:IAO_0000115>
        <oboInOwl:hasOBONamespace>GAZ</oboInOwl:hasOBONamespace>
        <oboInOwl:id>GAZ:00053554</oboInOwl:id>
        <rdfs:label>Emuruangogolak Volcano</rdfs:label>
    </owl:NamedIndividual>
    


    <!-- http://purl.obolibrary.org/obo/GAZ_00053555 -->

    <owl:NamedIndividual rdf:about="http://purl.obolibrary.org/obo/GAZ_00053555">
        <obo:RO_0001025 rdf:resource="http://purl.obolibrary.org/obo/GAZ_00000007"/>
        <obo:IAO_0000115>A trachytic shield volcano, the largest Quaternary volcano in the northern Gregory Rift, completely straddles the East African Rift. An impressive 5 x 8 km summit caldera with 300 m deep walls is thought to have formed about 63,000 years ago. Caldera formation is thought to have been incremental, related to eruption of the Kantenmening basaltic and trachytic lava flows. A series of summit-area lava benches formed by eruptions from circumferential fissures has produced a volcano morphologically similar to Galapagos Islands volcanoes. Northern, eastern, and southern flanks are cut by a prominent broad rift zone 10 km wide and 30 km long, dotted with numerous pyroclastic cones. Lava domes on the upper eastern flank formed during the late Pleistocene and early Holocene, until about 7 ka. Youthful parasitic cones abound on the caldera floor and on the northern and NE flanks; the youngest lava flows may be little more than a few hundred years old (Williams et al. 1984). Geothermal activity occurs within the caldera and on the upper eastern flanks.</obo:IAO_0000115>
        <oboInOwl:hasOBONamespace>GAZ</oboInOwl:hasOBONamespace>
        <oboInOwl:id>GAZ:00053555</oboInOwl:id>
        <rdfs:label>Silali Volcano</rdfs:label>
    </owl:NamedIndividual>
    


    <!-- http://purl.obolibrary.org/obo/GAZ_00053556 -->

    <owl:NamedIndividual rdf:about="http://purl.obolibrary.org/obo/GAZ_00053556">
        <obo:RO_0001025 rdf:resource="http://purl.obolibrary.org/obo/GAZ_00000007"/>
        <obo:IAO_0000115>A shield volcano in the Gregory Rift contains a small 1.5 km wide summit caldera. Eruption of large volumes of trachytic pyroclastic rocks around the end of the Pleistocene and the beginning of the Holocene formed a NW-trending ridge of pyroclastic cones across the summit region; collapse of this area formed the summit caldera and associated craters. A second large crater SE of the caldera is 0.5 x 1 km wide and contains a pumice cone. The summit caldera is narrowly breached on the north side, which has funneled post-caldera lava flows in this direction. The three youngest post-caldera pyroclastic cones on the NE flank may be only a few hundred years old. A series of viscous trachytic lava flows were erupted from vents on the volcano&apos;s lower flanks. Young fissure-fed basalts were also erupted to the south, between Paka and Korosi volcanoes. Surficial geothermal activity is widespread at Paka both within the summit caldera and on extensive portions of the northern flank.</obo:IAO_0000115>
        <oboInOwl:hasOBONamespace>GAZ</oboInOwl:hasOBONamespace>
        <oboInOwl:id>GAZ:00053556</oboInOwl:id>
        <rdfs:label>Paka Volcano</rdfs:label>
    </owl:NamedIndividual>
    


    <!-- http://purl.obolibrary.org/obo/GAZ_00053557 -->

    <owl:NamedIndividual rdf:about="http://purl.obolibrary.org/obo/GAZ_00053557">
        <obo:RO_0001025 rdf:resource="http://purl.obolibrary.org/obo/GAZ_00000007"/>
        <obo:IAO_0000115>A broad shield volcano west of Lake Bogoria that has been cut by spectacular grid faults along the west margin of the Gregory Rift. Geysers on the west margin of Lake Bogoria may be of tectonic origin.</obo:IAO_0000115>
        <oboInOwl:hasOBONamespace>GAZ</oboInOwl:hasOBONamespace>
        <oboInOwl:id>GAZ:00053557</oboInOwl:id>
        <rdfs:label>Bogoria Volcano</rdfs:label>
    </owl:NamedIndividual>
    


    <!-- http://purl.obolibrary.org/obo/GAZ_00053558 -->

    <owl:NamedIndividual rdf:about="http://purl.obolibrary.org/obo/GAZ_00053558">
        <obo:RO_0001025 rdf:resource="http://purl.obolibrary.org/obo/GAZ_00000007"/>
        <obo:IAO_0000115>A shield volcano that lies at the north end of Lake Baringo. Unlike other rift valley volcanoes, it does not contain a summit caldera. Lava domes on the northern flanks have fed trachytic lava flows. The major stage of Korosi volcanism spanned a period between 0.4 and 0.1 million years ago and included the eruption of voluminous fluid basaltic lava flows and pyroclastic cone formation along a NNE-trending fissure cutting across the axis of the shield volcano. This was followed by the eruption of trachytic lava domes and pumice/scoria cones. The youngest activity, consisting of fissure-fed basaltic lava flows on the lower northern flanks between Korosi and Paka, was probably coeval with the latest eruptions on Ol Kokwe to the south, which are only a few hundred to a few thousand years old (Dunkley et al. 1993). Fumaroles and hot steaming ground occur around the summit cones and NW flanks over an area of 30 sq km.</obo:IAO_0000115>
        <oboInOwl:hasOBONamespace>GAZ</oboInOwl:hasOBONamespace>
        <oboInOwl:id>GAZ:00053558</oboInOwl:id>
        <rdfs:label>Korosi Volcano</rdfs:label>
    </owl:NamedIndividual>
    


    <!-- http://purl.obolibrary.org/obo/GAZ_00053560 -->

    <owl:NamedIndividual rdf:about="http://purl.obolibrary.org/obo/GAZ_00053560">
        <obo:RO_0001025 rdf:resource="http://purl.obolibrary.org/obo/GAZ_00000007"/>
        <obo:IAO_0000115>A shield volcano that occupies the floor of the East African Rift. Construction of a 30 cu km shield volcano beginning about 200,000 years ago was followed by the eruption of two voluminous ash-flow tuffs, each preceded by major pumice falls.</obo:IAO_0000115>
        <oboInOwl:hasOBONamespace>GAZ</oboInOwl:hasOBONamespace>
        <oboInOwl:id>GAZ:00053560</oboInOwl:id>
        <rdfs:label>Menengai Volcano</rdfs:label>
    </owl:NamedIndividual>
    


    <!-- http://purl.obolibrary.org/obo/GAZ_00053565 -->

    <owl:NamedIndividual rdf:about="http://purl.obolibrary.org/obo/GAZ_00053565">
        <obo:RO_0001025 rdf:resource="http://purl.obolibrary.org/obo/GAZ_00000007"/>
        <obo:IAO_0000115>A volcanic field located between Lake Elmenteita and Eburru volcano, is an area of pyroclastic cones and lava flows of varying ages.</obo:IAO_0000115>
        <oboInOwl:hasOBONamespace>GAZ</oboInOwl:hasOBONamespace>
        <oboInOwl:id>GAZ:00053565</oboInOwl:id>
        <rdfs:label>Elmenteita Badlands</rdfs:label>
    </owl:NamedIndividual>
    


    <!-- http://purl.obolibrary.org/obo/GAZ_00053566 -->

    <owl:NamedIndividual rdf:about="http://purl.obolibrary.org/obo/GAZ_00053566">
        <obo:RO_0001025 rdf:resource="http://purl.obolibrary.org/obo/GAZ_00000007"/>
        <obo:IAO_0000115>A comple volcano that is elongated perpendicular to the Gregory Rift NW of Lake Naivasha. The 2856 m high, E-W-trending main edifice is eroded, but young partly vegetated rhyolitic domes occur on the east flank and are probably of Holocene age A prominent late-Pleistocene rhyolitic lava flow from a SE-flank vents extends almost to Lake Naivasha. Extensive fumarolic activity occurs at cinder cones and craters constructed along dominantly N-S-trending faults cutting the massif.</obo:IAO_0000115>
        <oboInOwl:hasOBONamespace>GAZ</oboInOwl:hasOBONamespace>
        <oboInOwl:id>GAZ:00053566</oboInOwl:id>
        <rdfs:label>Ol Doinyo Eburru Volcanic Complex</rdfs:label>
    </owl:NamedIndividual>
    


    <!-- http://purl.obolibrary.org/obo/GAZ_00053567 -->

    <owl:NamedIndividual rdf:about="http://purl.obolibrary.org/obo/GAZ_00053567">
        <obo:RO_0001025 rdf:resource="http://purl.obolibrary.org/obo/GAZ_00000007"/>
        <obo:IAO_0000115>A volcanic complex, located immediately south of Lake Naivasha and west of Longonot volcano, comprises up to 80 individual commenditic and other peralkaline rhyolitic centers. A thick, geochemically diverse basal complex is overlain by a dominantly silicic lava-dome and lava-flow complex active from about 20,000 years ago to the present. The youngest known eruption originated from the Ololbutot fissure on the SE side of the complex produced lava flows and a pumice flow and has a radiocarbon age of about 180 years. Fumarolic activity occurs at the Njorowa Gorge and at the Orengingnai and Olkaria (Orgaria) pumice cones.</obo:IAO_0000115>
        <oboInOwl:hasOBONamespace>GAZ</oboInOwl:hasOBONamespace>
        <oboInOwl:id>GAZ:00053567</oboInOwl:id>
        <rdfs:label>Olkaria Volcanic Complex</rdfs:label>
    </owl:NamedIndividual>
    


    <!-- http://purl.obolibrary.org/obo/GAZ_00053568 -->

    <owl:NamedIndividual rdf:about="http://purl.obolibrary.org/obo/GAZ_00053568">
        <obo:RO_0001025 rdf:resource="http://purl.obolibrary.org/obo/GAZ_00053569"/>
        <obo:IAO_0000115>A stratovolcano SE of Lake Naivasha in the Gregory Rift valley contains a 8 x 12 km caldera. Formation of the caldera accompanied large explosive eruptions about 21,000 years ago. A large central cone that was constructed within the caldera forms the 2776 m high summit of the volcano. The younger cone is truncated by a circular, 1.8 km wide crater. Post-caldera lavas are found on the caldera floor and the volcano&apos;s flanks, marking a late stage of effusive eruptions. A well-preserved satellitic cone is located on the NE flank.</obo:IAO_0000115>
        <oboInOwl:hasOBONamespace>GAZ</oboInOwl:hasOBONamespace>
        <oboInOwl:id>GAZ:00053568</oboInOwl:id>
        <rdfs:label>Mount Longonot</rdfs:label>
    </owl:NamedIndividual>
    


    <!-- http://purl.obolibrary.org/obo/GAZ_00053569 -->

    <owl:NamedIndividual rdf:about="http://purl.obolibrary.org/obo/GAZ_00053569">
        <obo:RO_0001025 rdf:resource="http://purl.obolibrary.org/obo/GAZ_00000007"/>
        <oboInOwl:hasOBONamespace>GAZ</oboInOwl:hasOBONamespace>
        <oboInOwl:id>GAZ:00053569</oboInOwl:id>
        <rdfs:label>Mount Longonot National Park</rdfs:label>
    </owl:NamedIndividual>
    


    <!-- http://purl.obolibrary.org/obo/GAZ_00053570 -->

    <owl:NamedIndividual rdf:about="http://purl.obolibrary.org/obo/GAZ_00053570">
        <obo:RO_0001025 rdf:resource="http://purl.obolibrary.org/obo/GAZ_00000007"/>
        <obo:IAO_0000115>A caldera of the Kenya rift, Suswa contains a prominent lava cone on the south side of its 8 x 12 km caldera. Suswa lies south of Longonot volcano and about 50 km WNW of the capital city of Nairobi. Construction of an early shield volcano was followed by eruption of voluminous Pleistocene pumice flows and lava flows that accompanied incremental formation of the caldera.</obo:IAO_0000115>
        <oboInOwl:hasOBONamespace>GAZ</oboInOwl:hasOBONamespace>
        <oboInOwl:id>GAZ:00053570</oboInOwl:id>
        <rdfs:label>Suswa Volcano</rdfs:label>
    </owl:NamedIndividual>
    


    <!-- http://purl.obolibrary.org/obo/GAZ_00053571 -->

    <owl:NamedIndividual rdf:about="http://purl.obolibrary.org/obo/GAZ_00053571">
        <obo:RO_0001025 rdf:resource="http://purl.obolibrary.org/obo/GAZ_00053570"/>
        <obo:IAO_0000115>A post-caldera lava cone.</obo:IAO_0000115>
        <oboInOwl:hasOBONamespace>GAZ</oboInOwl:hasOBONamespace>
        <oboInOwl:id>GAZ:00053571</oboInOwl:id>
        <rdfs:label>Ol Doinyo Onyoke</rdfs:label>
    </owl:NamedIndividual>
    


    <!-- http://purl.obolibrary.org/obo/GAZ_00053591 -->

    <owl:NamedIndividual rdf:about="http://purl.obolibrary.org/obo/GAZ_00053591">
        <obo:RO_0001025 rdf:resource="http://purl.obolibrary.org/obo/GAZ_00000007"/>
        <obo:IAO_0000115>A national park that protects Lake Nakuru, near Nakuru Town.</obo:IAO_0000115>
        <oboInOwl:hasOBONamespace>GAZ</oboInOwl:hasOBONamespace>
        <oboInOwl:id>GAZ:00053591</oboInOwl:id>
        <rdfs:label>Lake Nakuru National Park</rdfs:label>
    </owl:NamedIndividual>
    


    <!-- http://purl.obolibrary.org/obo/GAZ_00053598 -->

    <owl:NamedIndividual rdf:about="http://purl.obolibrary.org/obo/GAZ_00053598">
        <obo:RO_0001025 rdf:resource="http://purl.obolibrary.org/obo/GAZ_00051205"/>
        <obo:IAO_0000115>A stratovolcano that occupies an isolated location in the arid Danakil depression. It contains a large, central volcanotectonic depression that is open to the Zula Gulf and an isolated central cone. Jalua lies NW of basaltic lava flows of the Alid graben and south of the Zula Gulf.</obo:IAO_0000115>
        <oboInOwl:hasOBONamespace>GAZ</oboInOwl:hasOBONamespace>
        <oboInOwl:id>GAZ:00053598</oboInOwl:id>
        <rdfs:label>Jalua Volcano</rdfs:label>
    </owl:NamedIndividual>
    


    <!-- http://purl.obolibrary.org/obo/GAZ_00053599 -->

    <owl:NamedIndividual rdf:about="http://purl.obolibrary.org/obo/GAZ_00053599">
        <obo:RO_0001025 rdf:resource="http://purl.obolibrary.org/obo/GAZ_00051205"/>
        <obo:IAO_0000115>An isolated, dissected stratovolcano in the central Danakil depression. The volcano is elongated in an E-W direction perpendicular to the orientation of the Alid graben. Alid consists of a structural dome of uplifted sedimentary rocks, capped by basaltic-to-rhyolitic lava flows, that rises 700 m above the graben floor.</obo:IAO_0000115>
        <oboInOwl:hasOBONamespace>GAZ</oboInOwl:hasOBONamespace>
        <oboInOwl:id>GAZ:00053599</oboInOwl:id>
        <rdfs:label>Alid Volcano</rdfs:label>
    </owl:NamedIndividual>
    


    <!-- http://purl.obolibrary.org/obo/GAZ_00053600 -->

    <owl:NamedIndividual rdf:about="http://purl.obolibrary.org/obo/GAZ_00053600">
        <obo:RO_0001025 rdf:resource="http://purl.obolibrary.org/obo/GAZ_00053602"/>
        <obo:IAO_0000115>Numerous phreatic explosion craters dot the Salt Plain NNE of the Erta Ale Range in one of the lowest areas of the desolate Danakil depression. These craters mark Earth&apos;s lowest known subaerial volcanic vents.</obo:IAO_0000115>
        <oboInOwl:hasOBONamespace>GAZ</oboInOwl:hasOBONamespace>
        <oboInOwl:id>GAZ:00053600</oboInOwl:id>
        <rdfs:label>Dallol Volcano</rdfs:label>
    </owl:NamedIndividual>
    


    <!-- http://purl.obolibrary.org/obo/GAZ_00053601 -->

    <owl:NamedIndividual rdf:about="http://purl.obolibrary.org/obo/GAZ_00053601">
        <obo:RO_0001025 rdf:resource="http://purl.obolibrary.org/obo/GAZ_00053602"/>
        <obo:IAO_0000115>A prominent stratovolcano at the northern end of the Erta Ale Range. It is formed of interstratified lava flows and hyaloclastites. Fumarolic activity is continuing, and a small lake filled by boiling mud occupies the crater.</obo:IAO_0000115>
        <oboInOwl:hasOBONamespace>GAZ</oboInOwl:hasOBONamespace>
        <oboInOwl:id>GAZ:00053601</oboInOwl:id>
        <rdfs:label>Gada Ale Volcano</rdfs:label>
    </owl:NamedIndividual>
    


    <!-- http://purl.obolibrary.org/obo/GAZ_00053602 -->

    <owl:NamedIndividual rdf:about="http://purl.obolibrary.org/obo/GAZ_00053602">
        <obo:RO_0001025 rdf:resource="http://purl.obolibrary.org/obo/GAZ_00051205"/>
        <obo:IAO_0000115>An axial volcanic chain of the Afar Region, Ethiopia. It consists mostly of shield volcanoes.</obo:IAO_0000115>
        <oboInOwl:hasOBONamespace>GAZ</oboInOwl:hasOBONamespace>
        <oboInOwl:id>GAZ:00053602</oboInOwl:id>
        <rdfs:label>Erta Ale Range</rdfs:label>
    </owl:NamedIndividual>
    


    <!-- http://purl.obolibrary.org/obo/GAZ_00053603 -->

    <owl:NamedIndividual rdf:about="http://purl.obolibrary.org/obo/GAZ_00053603">
        <obo:RO_0001025 rdf:resource="http://purl.obolibrary.org/obo/GAZ_00053602"/>
        <obo:IAO_0000115>An active shield volcano located in the Afar Region of northeastern Ethiopia. It is the most active volcano in Ethiopia. The broad, 50 km wide volcano rises more than 600 m from below sea level in the barren Danakil depression.</obo:IAO_0000115>
        <oboInOwl:hasOBONamespace>GAZ</oboInOwl:hasOBONamespace>
        <oboInOwl:id>GAZ:00053603</oboInOwl:id>
        <rdfs:label>Erta Ale Volcano</rdfs:label>
    </owl:NamedIndividual>
    


    <!-- http://purl.obolibrary.org/obo/GAZ_00053604 -->

    <owl:NamedIndividual rdf:about="http://purl.obolibrary.org/obo/GAZ_00053604">
        <obo:RO_0001025 rdf:resource="http://purl.obolibrary.org/obo/GAZ_00053602"/>
        <obo:IAO_0000115>An elongated, 1031 m high stratovolcano located SW of Erta Ale volcano. It is the highest of the Erta Ale Range volcanoes and is located west of the axis of the range. In contrast to other volcanoes of the Erta Ale Range, Ale Bagu is mantled by basaltic pyroclastic rocks. Summit craters are elongated along a NNW-SSE trend. The main crater is a steep-walled, 750 x 450 m depression occupied by a steep-sided lava cone that has fed trachytic lava flows over the crater floor.</obo:IAO_0000115>
        <oboInOwl:hasOBONamespace>GAZ</oboInOwl:hasOBONamespace>
        <oboInOwl:id>GAZ:00053604</oboInOwl:id>
        <rdfs:label>Ale Bagu Volcano</rdfs:label>
    </owl:NamedIndividual>
    


    <!-- http://purl.obolibrary.org/obo/GAZ_00053605 -->

    <owl:NamedIndividual rdf:about="http://purl.obolibrary.org/obo/GAZ_00053605">
        <obo:RO_0001025 rdf:resource="http://purl.obolibrary.org/obo/GAZ_00053602"/>
        <obo:IAO_0000115>A small, but steep-sided conical stratovolcano that rises 300 m above surrounding lava fields SE of Alu volcano. This morphology, unusual for the Erta Ale Range volcanoes, results from the extrusion of viscous, silicic lava flows with primary slopes up to about 35 degrees. These silicic flows extend primarily to the east; on the west they are blocked by walls of a horst structure along the crest of the Erta Ale range.</obo:IAO_0000115>
        <oboInOwl:hasOBONamespace>GAZ</oboInOwl:hasOBONamespace>
        <oboInOwl:id>GAZ:00053605</oboInOwl:id>
        <rdfs:label>Dalaffilla Volcano</rdfs:label>
    </owl:NamedIndividual>
    


    <!-- http://purl.obolibrary.org/obo/GAZ_00053606 -->

    <owl:NamedIndividual rdf:about="http://purl.obolibrary.org/obo/GAZ_00053606">
        <obo:RO_0001025 rdf:resource="http://purl.obolibrary.org/obo/GAZ_00053602"/>
        <obo:IAO_0000115>A system of volcanic fissures, located in Ethiopia. The fissures have produced silicic lava flows, and other fissures south of the volcano have formed huge youthful basaltic lava flows, which enlarge to the north as far as Lake Bakili. There is major fumarolic motion, which are located on frequent corresponding faults, some of which gave a lift up to 100 m.</obo:IAO_0000115>
        <oboInOwl:hasOBONamespace>GAZ</oboInOwl:hasOBONamespace>
        <oboInOwl:id>GAZ:00053606</oboInOwl:id>
        <rdfs:label>Alu Fissure Vents</rdfs:label>
    </owl:NamedIndividual>
    


    <!-- http://purl.obolibrary.org/obo/GAZ_00053607 -->

    <owl:NamedIndividual rdf:about="http://purl.obolibrary.org/obo/GAZ_00053607">
        <obo:RO_0001025 rdf:resource="http://purl.obolibrary.org/obo/GAZ_00053602"/>
        <obo:IAO_0000115>A complex stratovolcano located near the center of the Erta Ale Range. The earliest activity formed submarine lava flows partially covered by Quaternary reef deposits. An embryonic shield volcano is located on the SW side of the complex and is cut by curvilinear faults; youthful chains of spatter cones follow this same curvilinear pattern and form concentric semi-circles. The 668 m high summit of the Borale Ale complex is located on the NE side of the massif and consists of a silicic stratovolcano that is the largest of the Erte Ale Range. It has produced steep-sided viscous lava flows that have traveled up to 5 km from the volcano. Strong fumarolic activity occurs within a 300-m-wide summit crater.</obo:IAO_0000115>
        <oboInOwl:hasOBONamespace>GAZ</oboInOwl:hasOBONamespace>
        <oboInOwl:id>GAZ:00053607</oboInOwl:id>
        <rdfs:label>Borale Ale Volcano</rdfs:label>
    </owl:NamedIndividual>
    


    <!-- http://purl.obolibrary.org/obo/GAZ_00053608 -->

    <owl:NamedIndividual rdf:about="http://purl.obolibrary.org/obo/GAZ_00053608">
        <obo:RO_0001025 rdf:resource="http://purl.obolibrary.org/obo/GAZ_00053602"/>
        <obo:IAO_0000115>A shield volcano where tectonism has created a graben at the 521 m high summit. A symmetrical scoria cone with a 200-m-wide crater displaying fumarolic activity occupies the center of the graben. An older shield volcano is covered on the north by recent fissure-fed lava flows. Lava flows from the axial portion of a fissure system extending to the south have reached the floor of the Giulietti Plain south of the Erta Ale Range. The open fissures extend for more than 10 km and are lined with dozens of small spatter cones and pit craters.</obo:IAO_0000115>
        <oboInOwl:hasOBONamespace>GAZ</oboInOwl:hasOBONamespace>
        <oboInOwl:id>GAZ:00053608</oboInOwl:id>
        <rdfs:label>Hayli Gubbi Volcano</rdfs:label>
    </owl:NamedIndividual>
    


    <!-- http://purl.obolibrary.org/obo/GAZ_00053609 -->

    <owl:NamedIndividual rdf:about="http://purl.obolibrary.org/obo/GAZ_00053609">
        <obo:RO_0001025 rdf:resource="http://purl.obolibrary.org/obo/GAZ_00051205"/>
        <obo:IAO_0000115>A stratovolcano located east of the Erta Ale Range and south of the crystalline basement rocks of the Danakil Alps. It is a large volcanic massif that rises to 1625 m above the western shore of the Red Sea. About 20 small cinder cones are located at the summit, and extensive basaltic lava fields to the north and NE, known as the Edd lava field, cover an area of 2700 km2 and reach the Red Sea coast.</obo:IAO_0000115>
        <oboInOwl:hasOBONamespace>GAZ</oboInOwl:hasOBONamespace>
        <oboInOwl:id>GAZ:00053609</oboInOwl:id>
        <rdfs:label>Dubbi Volcano</rdfs:label>
    </owl:NamedIndividual>
    


    <!-- http://purl.obolibrary.org/obo/GAZ_00053610 -->

    <owl:NamedIndividual rdf:about="http://purl.obolibrary.org/obo/GAZ_00053610">
        <obo:RO_0001025 rdf:resource="http://purl.obolibrary.org/obo/GAZ_00051205"/>
        <obo:IAO_0000115>A stratovolcano in the Danakil depression of northern Ethiopia and Eritrea. Located at the SE end of the Danakil Alps, Nabro lies in the Danakil horst. Nabro is the most prominent and NE-most of three volcanoes with large summit calderas aligned in a NE-SW direction SW of Dubbi volcano. These three volcanoes, along with Sork Ale volcano, collectively comprise the Bidu volcanic complex. The complex Nabro stratovolcano is truncated by nested calderas, 8 and 5 km in diameter. The larger caldera is widely breached to the SW. Nabro was constructed primarily of trachytic lava flows and pyroclastics. Post-caldera rhyolitic obsidian domes and basaltic lava flows were erupted inside the caldera and on its flanks.</obo:IAO_0000115>
        <oboInOwl:hasOBONamespace>GAZ</oboInOwl:hasOBONamespace>
        <oboInOwl:id>GAZ:00053610</oboInOwl:id>
        <rdfs:label>Nabro Volcano</rdfs:label>
    </owl:NamedIndividual>
    


    <!-- http://purl.obolibrary.org/obo/GAZ_00053619 -->

    <owl:NamedIndividual rdf:about="http://purl.obolibrary.org/obo/GAZ_00053619">
        <obo:RO_0001025 rdf:resource="http://purl.obolibrary.org/obo/GAZ_00051205"/>
        <obo:IAO_0000115>A saline lake in northern Ethiopia. Located in the Administrative Zone 2, it is one of the lakes of the Afar Depression.</obo:IAO_0000115>
        <oboInOwl:hasOBONamespace>GAZ</oboInOwl:hasOBONamespace>
        <oboInOwl:id>GAZ:00053619</oboInOwl:id>
        <rdfs:label>Lake Afrera</rdfs:label>
    </owl:NamedIndividual>
    


    <!-- http://purl.obolibrary.org/obo/GAZ_00053620 -->

    <owl:NamedIndividual rdf:about="http://purl.obolibrary.org/obo/GAZ_00053620">
        <obo:RO_0001025 rdf:resource="http://purl.obolibrary.org/obo/GAZ_00053632"/>
        <obo:IAO_0000115>A stratovolcano that rises above the eastern shore of Lake Afrera, also known as Lake Giulietti. The upper part of the 812 m high conical volcano consists of trachytic lava flows overlying older basaltic flows. Young pantelleritic obsidian domes south of the volcano are the probable source of rounded pumice fragments found around Lake Afrera.</obo:IAO_0000115>
        <oboInOwl:hasOBONamespace>GAZ</oboInOwl:hasOBONamespace>
        <oboInOwl:id>GAZ:00053620</oboInOwl:id>
        <rdfs:label>Borawli Volcano</rdfs:label>
    </owl:NamedIndividual>
    


    <!-- http://purl.obolibrary.org/obo/GAZ_00053622 -->

    <owl:NamedIndividual rdf:about="http://purl.obolibrary.org/obo/GAZ_00053622">
        <obo:RO_0001025 rdf:resource="http://purl.obolibrary.org/obo/GAZ_00051205"/>
        <obo:IAO_0000115>An 1815 m high stratovolcano located well to the west of the Danakil depression at the foot of the regional Ethiopian scarp. The volcano is situated between two large horsts of uplifted basement blocks. A large trachytic and rhyolitic stratovolcano at the center of the Ma Alalta complex contains nested oval-shaped summit calderas, 8 x 5 km and 5 x 2.5 km wide. Ignimbrite deposits, perhaps associated with formation of the larger caldera, extend beyond the volcano primarily to the NE and SE. Young basaltic lava flows were erupted on the NW, SE, and eastern flanks of the volcano. Recent silicic activity has produced pantelleritic obsidian domes and lava flows on the volcano&apos;s southern flank. Fumarolic activity continues at one of the domes.</obo:IAO_0000115>
        <oboInOwl:hasOBONamespace>GAZ</oboInOwl:hasOBONamespace>
        <oboInOwl:id>GAZ:00053622</oboInOwl:id>
        <rdfs:label>Ma Alalta Volcano</rdfs:label>
    </owl:NamedIndividual>
    


    <!-- http://purl.obolibrary.org/obo/GAZ_00053623 -->

    <owl:NamedIndividual rdf:about="http://purl.obolibrary.org/obo/GAZ_00053623">
        <obo:RO_0001025 rdf:resource="http://purl.obolibrary.org/obo/GAZ_00051205"/>
        <obo:IAO_0000115>A shield volcano covers an area of 2700 km2 in the western Danakil depression SW of Lake Afrera. A series of very recent craters is aligned along the NNW-trending axis of the basaltic-to-trachytic shield. The Alayta lava field, covered by very fresh lava flows, was erupted from N-S-trending fissures along the east side of the shield volcano and laps up against the western flank of Afdera volcano.</obo:IAO_0000115>
        <oboInOwl:hasOBONamespace>GAZ</oboInOwl:hasOBONamespace>
        <oboInOwl:id>GAZ:00053623</oboInOwl:id>
        <rdfs:label>Alayta Volcano</rdfs:label>
    </owl:NamedIndividual>
    


    <!-- http://purl.obolibrary.org/obo/GAZ_00053624 -->

    <owl:NamedIndividual rdf:about="http://purl.obolibrary.org/obo/GAZ_00053624">
        <obo:RO_0001025 rdf:resource="http://purl.obolibrary.org/obo/GAZ_00051205"/>
        <obo:IAO_0000115>A Holocene stratovolcanic massif forming an axial range of the Afar depression SSW of the Alayta massif. Pantelleritic obsidian flows, lava domes, and pumice cones form the summit and upper flanks of the volcano, which rises above the Teru Plain and was built over a base of basaltic-to-trachytic lava flows of a shield volcano. Late-stage basaltic fissure eruptions occurred at the NW base of the volcano. Abundant fumaroles are located along the crest of the volcano and extend NE towards Alayta volcano.</obo:IAO_0000115>
        <oboInOwl:hasOBONamespace>GAZ</oboInOwl:hasOBONamespace>
        <oboInOwl:id>GAZ:00053624</oboInOwl:id>
        <rdfs:label>Dabbahu Volcano</rdfs:label>
    </owl:NamedIndividual>
    


    <!-- http://purl.obolibrary.org/obo/GAZ_00053625 -->

    <owl:NamedIndividual rdf:about="http://purl.obolibrary.org/obo/GAZ_00053625">
        <obo:RO_0001025 rdf:resource="http://purl.obolibrary.org/obo/GAZ_00051205"/>
        <obo:IAO_0000115>A shield volcano that was constructed along an offshoot of the Ethiopian escarpment, SW of the Teru plain. In contrast to structural trends in other parts of Afar, Dabbayra consists of a basaltic shield volcano elongated in an ENE-WSW direction. The only silicic volcanic rocks are a NNW-trending line of lava domes and lava flows near the crest of the 1302 m high volcano.</obo:IAO_0000115>
        <oboInOwl:hasOBONamespace>GAZ</oboInOwl:hasOBONamespace>
        <oboInOwl:id>GAZ:00053625</oboInOwl:id>
        <rdfs:label>Dabbayra Volcano</rdfs:label>
    </owl:NamedIndividual>
    


    <!-- http://purl.obolibrary.org/obo/GAZ_00053626 -->

    <owl:NamedIndividual rdf:about="http://purl.obolibrary.org/obo/GAZ_00053626">
        <obo:RO_0001025 rdf:resource="http://purl.obolibrary.org/obo/GAZ_00051205"/>
        <obo:IAO_0000115>A complex of shield volcanoes located in the Kalo plain, SSE of Dabbahu volcano. The massive complex is 105 km long and 20-30 km wide, and represents an uplifted segment of a mid-ocean ridge spreading center. A small basaltic shield volcano is located at the northern end of the complex, south of which is an area of abundant fissure-fed lava flows. Two basaltic shield volcanoes, the largest of which is Unda Hararo, occupy the center of the complex. The dominant part of the complex lies to the south, where the Gumatmali-Gablaytu fissure system is located. Voluminous fluid lava flows issued from these NNW-trending fissures, and solidified lava lakes occupy two large craters. The small Gablaytu shield volcano forms the SE-most end of the Manda Hararo complex. Lava flows from Gablaytu and from Manda overlie 8000-year-old sediments. Hot springs and fumaroles occur around Daorre lake.</obo:IAO_0000115>
        <oboInOwl:hasOBONamespace>GAZ</oboInOwl:hasOBONamespace>
        <oboInOwl:id>GAZ:00053626</oboInOwl:id>
        <rdfs:label>Manda Hararo Volcanic Complex</rdfs:label>
    </owl:NamedIndividual>
    


    <!-- http://purl.obolibrary.org/obo/GAZ_00053627 -->

    <owl:NamedIndividual rdf:about="http://purl.obolibrary.org/obo/GAZ_00053627">
        <obo:RO_0001025 rdf:resource="http://purl.obolibrary.org/obo/GAZ_00053626"/>
        <obo:IAO_0000115>A shield volcano.</obo:IAO_0000115>
        <oboInOwl:hasOBONamespace>GAZ</oboInOwl:hasOBONamespace>
        <oboInOwl:id>GAZ:00053627</oboInOwl:id>
        <rdfs:label>Gablaytu Volcano</rdfs:label>
    </owl:NamedIndividual>
    


    <!-- http://purl.obolibrary.org/obo/GAZ_00053628 -->

    <owl:NamedIndividual rdf:about="http://purl.obolibrary.org/obo/GAZ_00053628">
        <obo:RO_0001025 rdf:resource="http://purl.obolibrary.org/obo/GAZ_00053626"/>
        <obo:IAO_0000115>A fissure system.</obo:IAO_0000115>
        <oboInOwl:hasOBONamespace>GAZ</oboInOwl:hasOBONamespace>
        <oboInOwl:id>GAZ:00053628</oboInOwl:id>
        <rdfs:label>Gumatmali-Gablaytu Fissure System</rdfs:label>
    </owl:NamedIndividual>
    


    <!-- http://purl.obolibrary.org/obo/GAZ_00053629 -->

    <owl:NamedIndividual rdf:about="http://purl.obolibrary.org/obo/GAZ_00053629">
        <obo:RO_0001025 rdf:resource="http://purl.obolibrary.org/obo/GAZ_00053626"/>
        <obo:IAO_0000115>A basaltic shield volcano.</obo:IAO_0000115>
        <oboInOwl:hasOBONamespace>GAZ</oboInOwl:hasOBONamespace>
        <oboInOwl:id>GAZ:00053629</oboInOwl:id>
        <rdfs:label>Unda Hararo Volcano</rdfs:label>
    </owl:NamedIndividual>
    


    <!-- http://purl.obolibrary.org/obo/GAZ_00053630 -->

    <owl:NamedIndividual rdf:about="http://purl.obolibrary.org/obo/GAZ_00053630">
        <obo:RO_0001025 rdf:resource="http://purl.obolibrary.org/obo/GAZ_00051205"/>
        <obo:IAO_0000115>A small 930 m high alkali rhyolitic stratovolcano located in the western Afar near the Ethiopian escarpment, NE of Dessye.</obo:IAO_0000115>
        <oboInOwl:hasOBONamespace>GAZ</oboInOwl:hasOBONamespace>
        <oboInOwl:id>GAZ:00053630</oboInOwl:id>
        <rdfs:label>Groppo Volcano</rdfs:label>
    </owl:NamedIndividual>
    


    <!-- http://purl.obolibrary.org/obo/GAZ_00053631 -->

    <owl:NamedIndividual rdf:about="http://purl.obolibrary.org/obo/GAZ_00053631">
        <obo:RO_0001025 rdf:resource="http://purl.obolibrary.org/obo/GAZ_00051205"/>
        <obo:IAO_0000115>A shield volcano that lies in the Saha Plain, SE of the Manda Hararo complex in the South Danakil region. Wind-blown sand fills the summit crater of the young basaltic volcano. Initial subaqueous activity occurred along NNW-trending fissures. Fumarolic activity observed in the 1930s was not seen during field work in the 1970s.</obo:IAO_0000115>
        <oboInOwl:hasOBONamespace>GAZ</oboInOwl:hasOBONamespace>
        <oboInOwl:id>GAZ:00053631</oboInOwl:id>
        <rdfs:label>Kurub Volcano</rdfs:label>
    </owl:NamedIndividual>
    


    <!-- http://purl.obolibrary.org/obo/GAZ_00053632 -->

    <owl:NamedIndividual rdf:about="http://purl.obolibrary.org/obo/GAZ_00053632">
        <obo:RO_0001025 rdf:resource="http://purl.obolibrary.org/obo/GAZ_00051205"/>
        <obo:IAO_0000115>A group of rhyolitic lava domes on the floor of the southern Kali plain, north of Aysa&apos;iyta.</obo:IAO_0000115>
        <oboInOwl:hasOBONamespace>GAZ</oboInOwl:hasOBONamespace>
        <oboInOwl:id>GAZ:00053632</oboInOwl:id>
        <rdfs:label>Borawli Volcanic Complex</rdfs:label>
    </owl:NamedIndividual>
    


    <!-- http://purl.obolibrary.org/obo/GAZ_00053663 -->

    <owl:NamedIndividual rdf:about="http://purl.obolibrary.org/obo/GAZ_00053663">
        <obo:RO_0001025 rdf:resource="http://purl.obolibrary.org/obo/GAZ_00000007"/>
        <obo:IAO_0000115>A freshwater lake in the Oromia Region of Ethiopia, about 100 km south of the capital, Addis Ababa, on the border between the Misraq Shewa and Arsi Zones. It is located in the Great Rift Valley at an elevation of 1,585 meters to the east of Lake Abijatta.</obo:IAO_0000115>
        <oboInOwl:hasOBONamespace>GAZ</oboInOwl:hasOBONamespace>
        <oboInOwl:id>GAZ:00053663</oboInOwl:id>
        <rdfs:label>Lake Langano</rdfs:label>
    </owl:NamedIndividual>
    


    <!-- http://purl.obolibrary.org/obo/GAZ_00053667 -->

    <owl:NamedIndividual rdf:about="http://purl.obolibrary.org/obo/GAZ_00053667">
        <obo:RO_0001025 rdf:resource="http://purl.obolibrary.org/obo/GAZ_00000007"/>
        <obo:IAO_0000115>A lake that is surrounded by hot springs filled with boiling water, and the earth surrounding the lake is filled with cracks due to erosion and earthquakes. Due to steam rising from the boiling water in the springs, the atmosphere around the lake is relatively foggy.</obo:IAO_0000115>
        <oboInOwl:hasOBONamespace>GAZ</oboInOwl:hasOBONamespace>
        <oboInOwl:id>GAZ:00053667</oboInOwl:id>
        <rdfs:label>Lake Shala</rdfs:label>
    </owl:NamedIndividual>
    


    <!-- http://purl.obolibrary.org/obo/GAZ_00053668 -->

    <owl:NamedIndividual rdf:about="http://purl.obolibrary.org/obo/GAZ_00053668">
        <obo:RO_0001025 rdf:resource="http://purl.obolibrary.org/obo/GAZ_00053667"/>
        <obo:IAO_0000115>An island in Lake Shala.</obo:IAO_0000115>
        <oboInOwl:hasOBONamespace>GAZ</oboInOwl:hasOBONamespace>
        <oboInOwl:id>GAZ:00053668</oboInOwl:id>
        <rdfs:label>Pelican Island</rdfs:label>
    </owl:NamedIndividual>
    


    <!-- http://purl.obolibrary.org/obo/GAZ_00053675 -->

    <owl:NamedIndividual rdf:about="http://purl.obolibrary.org/obo/GAZ_00053675">
        <obo:RO_0001025 rdf:resource="http://purl.obolibrary.org/obo/GAZ_00000007"/>
        <obo:IAO_0000115>A lake in the Southern Nations, Nationalities, and Peoples Region of southern Ethiopia. It is located in the Great Rift Valley at an elevation of 1,235 meters. It is just to the south of Lake Abaya and the city of Arba Minch, and east of the Guge Mountains. Lake Chamo does not always have an outflow, but in some years, it overflows into the Sagan River. In some years, it is fed by overflow from Lake Abaya.</obo:IAO_0000115>
        <oboInOwl:hasOBONamespace>GAZ</oboInOwl:hasOBONamespace>
        <oboInOwl:id>GAZ:00053675</oboInOwl:id>
        <rdfs:label>Lake Chamo</rdfs:label>
    </owl:NamedIndividual>
    


    <!-- http://purl.obolibrary.org/obo/GAZ_00053679 -->

    <owl:NamedIndividual rdf:about="http://purl.obolibrary.org/obo/GAZ_00053679">
        <obo:RO_0001025 rdf:resource="http://purl.obolibrary.org/obo/GAZ_00051205"/>
        <obo:IAO_0000115>A vegetated rhyolitic stratovolcano, located south of the Asbahri plain in the southern Afar region. On its eastern side, 2145 m high Ayelu is cut by regional faults and is overlain by ignimbrites erupted from Adwa volcano immediately to the east. Ayelu was constructed by a series of thick rhyolitic lava flows, creating a higher and steeper-sided volcano than its neighbor Adwa. Hot springs are located on the western flank of Ayelu.</obo:IAO_0000115>
        <oboInOwl:hasOBONamespace>GAZ</oboInOwl:hasOBONamespace>
        <oboInOwl:id>GAZ:00053679</oboInOwl:id>
        <rdfs:label>Mount Ayalu</rdfs:label>
    </owl:NamedIndividual>
    


    <!-- http://purl.obolibrary.org/obo/GAZ_00057510 -->

    <owl:NamedIndividual rdf:about="http://purl.obolibrary.org/obo/GAZ_00057510">
        <obo:RO_0001025 rdf:resource="http://purl.obolibrary.org/obo/GAZ_00051205"/>
        <obo:IAO_0000115>An endorheic saline lake lying on the Ethiopia-Djibouti border, and is one of a chain of six connected lakes which also includes (from north to south) lakes Gargori, Laitali, Gummare, Bario and Afambo. Lake Abbe is the ultimate destination of the waters of the Awash River. Lake Abbe is at the central point of the Afar Depression, where three pieces of the earth&apos;s crust meet. On the northwest shore rises Dama Ali, a volcanic mountain.</obo:IAO_0000115>
        <oboInOwl:hasOBONamespace>GAZ</oboInOwl:hasOBONamespace>
        <oboInOwl:id>GAZ:00057510</oboInOwl:id>
        <rdfs:label>Lake Abbe</rdfs:label>
    </owl:NamedIndividual>
    


    <!-- http://purl.obolibrary.org/obo/GAZ_00058384 -->

    <owl:NamedIndividual rdf:about="http://purl.obolibrary.org/obo/GAZ_00058384">
        <obo:RO_0001025 rdf:resource="http://purl.obolibrary.org/obo/GAZ_00008742"/>
        <obo:IAO_0000115>A lake that was drained in the 1950s, but is now being regenerated.</obo:IAO_0000115>
        <oboInOwl:hasOBONamespace>GAZ</oboInOwl:hasOBONamespace>
        <oboInOwl:id>GAZ:00058384</oboInOwl:id>
        <rdfs:label>Lake Hulah</rdfs:label>
    </owl:NamedIndividual>
    


    <!-- http://purl.obolibrary.org/obo/GAZ_00058395 -->

    <owl:NamedIndividual rdf:about="http://purl.obolibrary.org/obo/GAZ_00058395">
        <obo:RO_0001025 rdf:resource="http://purl.obolibrary.org/obo/GAZ_00058396"/>
        <obo:IAO_0000115>An artificial lake located in the southern region of the Beqaa Valley. Made by damming the Litani River.</obo:IAO_0000115>
        <oboInOwl:hasOBONamespace>GAZ</oboInOwl:hasOBONamespace>
        <oboInOwl:id>GAZ:00058395</oboInOwl:id>
        <rdfs:label>Lake Qaraoun</rdfs:label>
    </owl:NamedIndividual>
    


    <!-- http://purl.obolibrary.org/obo/GAZ_00058396 -->

    <owl:NamedIndividual rdf:about="http://purl.obolibrary.org/obo/GAZ_00058396">
        <obo:RO_0001025 rdf:resource="http://purl.obolibrary.org/obo/GAZ_00044906"/>
        <obo:IAO_0000115>A river that rises west of Baalbek in the fertile Beqaa Valley and empties in the Mediterranean Sea north of Tyre.</obo:IAO_0000115>
        <oboInOwl:hasOBONamespace>GAZ</oboInOwl:hasOBONamespace>
        <oboInOwl:id>GAZ:00058396</oboInOwl:id>
        <rdfs:label>Litani River</rdfs:label>
    </owl:NamedIndividual>
    


    <!-- http://purl.obolibrary.org/obo/GAZ_00058780 -->

    <owl:NamedIndividual rdf:about="http://purl.obolibrary.org/obo/GAZ_00058780">
        <obo:RO_0001025 rdf:resource="http://purl.obolibrary.org/obo/GAZ_00058782"/>
        <obo:IAO_0000115>A lake lagoon in Zambia. It is the largest of several lagoons in the Luapula River swamps south of Lake Mweru, in the Luapula Province of Zambia.</obo:IAO_0000115>
        <oboInOwl:hasOBONamespace>GAZ</oboInOwl:hasOBONamespace>
        <oboInOwl:id>GAZ:00058780</oboInOwl:id>
        <rdfs:label>Mofwe Lagoon</rdfs:label>
    </owl:NamedIndividual>
    


    <!-- http://purl.obolibrary.org/obo/GAZ_00058781 -->

    <owl:NamedIndividual rdf:about="http://purl.obolibrary.org/obo/GAZ_00058781">
        <obo:IAO_0000115>A river that drains the northern Zambian plateau north of Kawambwa and flows west into the Luapula valley. It enters the Luapula swamps near the Mofwe Lagoon.</obo:IAO_0000115>
        <oboInOwl:hasOBONamespace>GAZ</oboInOwl:hasOBONamespace>
        <oboInOwl:id>GAZ:00058781</oboInOwl:id>
        <rdfs:label>Mbereshi River</rdfs:label>
    </owl:NamedIndividual>
    


    <!-- http://purl.obolibrary.org/obo/GAZ_00058782 -->

    <owl:NamedIndividual rdf:about="http://purl.obolibrary.org/obo/GAZ_00058782">
        <obo:IAO_0000115>Swamps that stretch along the last 100 km of the Luapula River before it reaches the Lake Mweru, and for much of that they are 30 km wide, covering and area of about 2500 km2. There are four inhabited islands in the DR Congo part of the delta, including the largest in the system which is connected to dry land in the dry season. Zambia has three inhabited islands in the delta including Chisenga Island. The are also many lagoons, the largest of which is Mofwe Lagoon on the Zambian side.</obo:IAO_0000115>
        <oboInOwl:hasOBONamespace>GAZ</oboInOwl:hasOBONamespace>
        <oboInOwl:id>GAZ:00058782</oboInOwl:id>
        <rdfs:label>Luapula Swamps</rdfs:label>
    </owl:NamedIndividual>
    


    <!-- http://purl.obolibrary.org/obo/GAZ_00058783 -->

    <owl:NamedIndividual rdf:about="http://purl.obolibrary.org/obo/GAZ_00058783">
        <obo:RO_0001025 rdf:resource="http://purl.obolibrary.org/obo/GAZ_00058782"/>
        <obo:IAO_0000115>A Zambian island in the Luapula Swamps.</obo:IAO_0000115>
        <oboInOwl:hasOBONamespace>GAZ</oboInOwl:hasOBONamespace>
        <oboInOwl:id>GAZ:00058783</oboInOwl:id>
        <rdfs:label>Chisenga Island</rdfs:label>
    </owl:NamedIndividual>
    


    <!-- http://purl.obolibrary.org/obo/GAZ_00058786 -->

    <owl:NamedIndividual rdf:about="http://purl.obolibrary.org/obo/GAZ_00058786">
        <obo:RO_0001025 rdf:resource="http://purl.obolibrary.org/obo/GAZ_00015397"/>
        <obo:IAO_0000115>A lake that lies in south western Uganda between Kisoro and Kabale close to the border with Rwanda.</obo:IAO_0000115>
        <oboInOwl:hasOBONamespace>GAZ</oboInOwl:hasOBONamespace>
        <oboInOwl:id>GAZ:00058786</oboInOwl:id>
        <rdfs:label>Lake Bunyonyi</rdfs:label>
    </owl:NamedIndividual>
    


    <!-- http://purl.obolibrary.org/obo/GAZ_00058787 -->

    <owl:NamedIndividual rdf:about="http://purl.obolibrary.org/obo/GAZ_00058787">
        <obo:RO_0001025 rdf:resource="http://purl.obolibrary.org/obo/GAZ_00058786"/>
        <obo:IAO_0000115>An island in Lake Bunyonyi.</obo:IAO_0000115>
        <oboInOwl:hasOBONamespace>GAZ</oboInOwl:hasOBONamespace>
        <oboInOwl:id>GAZ:00058787</oboInOwl:id>
        <rdfs:label>Akampene Island</rdfs:label>
    </owl:NamedIndividual>
    


    <!-- http://purl.obolibrary.org/obo/GAZ_00058788 -->

    <owl:NamedIndividual rdf:about="http://purl.obolibrary.org/obo/GAZ_00058788">
        <obo:RO_0001025 rdf:resource="http://purl.obolibrary.org/obo/GAZ_00058786"/>
        <obo:IAO_0000115>An island in Lake Bunyonyi.</obo:IAO_0000115>
        <oboInOwl:hasOBONamespace>GAZ</oboInOwl:hasOBONamespace>
        <oboInOwl:id>GAZ:00058788</oboInOwl:id>
        <rdfs:label>Bucuranuka Island</rdfs:label>
    </owl:NamedIndividual>
    


    <!-- http://purl.obolibrary.org/obo/GAZ_00058789 -->

    <owl:NamedIndividual rdf:about="http://purl.obolibrary.org/obo/GAZ_00058789">
        <obo:RO_0001025 rdf:resource="http://purl.obolibrary.org/obo/GAZ_00058786"/>
        <obo:IAO_0000115>An island in Lake Bunyonyi.</obo:IAO_0000115>
        <oboInOwl:hasOBONamespace>GAZ</oboInOwl:hasOBONamespace>
        <oboInOwl:id>GAZ:00058789</oboInOwl:id>
        <rdfs:label>Bwama and Njuyeera Island</rdfs:label>
    </owl:NamedIndividual>
    


    <!-- http://purl.obolibrary.org/obo/GAZ_00058790 -->

    <owl:NamedIndividual rdf:about="http://purl.obolibrary.org/obo/GAZ_00058790">
        <obo:RO_0001025 rdf:resource="http://purl.obolibrary.org/obo/GAZ_00058786"/>
        <obo:IAO_0000115>An island in Lake Bunyonyi.</obo:IAO_0000115>
        <oboInOwl:hasOBONamespace>GAZ</oboInOwl:hasOBONamespace>
        <oboInOwl:id>GAZ:00058790</oboInOwl:id>
        <rdfs:label>Bushara Island</rdfs:label>
    </owl:NamedIndividual>
    


    <!-- http://purl.obolibrary.org/obo/GAZ_00058791 -->

    <owl:NamedIndividual rdf:about="http://purl.obolibrary.org/obo/GAZ_00058791">
        <obo:RO_0001025 rdf:resource="http://purl.obolibrary.org/obo/GAZ_00000007"/>
        <obo:RO_0001025 rdf:resource="http://purl.obolibrary.org/obo/GAZ_00015355"/>
        <obo:IAO_0000115>A polymictic shallow lake complex of Uganda, about 1,720 km2 in area and at an elevation of 914 m. The Victoria Nile flows through the lake on its way from Lake Victoria to Lake Albert. The main inflow from Lake Victoria is regulated by the Nalubaale Power Station in Jinja. Another source of water is the Mount Elgon region on the border between Uganda and Kenya.</obo:IAO_0000115>
        <oboInOwl:hasOBONamespace>GAZ</oboInOwl:hasOBONamespace>
        <oboInOwl:id>GAZ:00058791</oboInOwl:id>
        <rdfs:label>Lake Kyoga</rdfs:label>
    </owl:NamedIndividual>
    


    <!-- http://purl.obolibrary.org/obo/GAZ_00058792 -->

    <owl:NamedIndividual rdf:about="http://purl.obolibrary.org/obo/GAZ_00058792">
        <obo:RO_0001025 rdf:resource="http://purl.obolibrary.org/obo/GAZ_00000007"/>
        <obo:IAO_0000115>A lake in Uganda. It drains to the SW into Lake Edward through the Kazinga Channel.</obo:IAO_0000115>
        <oboInOwl:hasOBONamespace>GAZ</oboInOwl:hasOBONamespace>
        <oboInOwl:id>GAZ:00058792</oboInOwl:id>
        <rdfs:label>Lake George</rdfs:label>
    </owl:NamedIndividual>
    


    <!-- http://purl.obolibrary.org/obo/GAZ_00058793 -->

    <owl:NamedIndividual rdf:about="http://purl.obolibrary.org/obo/GAZ_00058793">
        <obo:RO_0001025 rdf:resource="http://purl.obolibrary.org/obo/GAZ_00015388"/>
        <obo:RO_0001025 rdf:resource="http://purl.obolibrary.org/obo/GAZ_00015393"/>
        <obo:IAO_0000115>A lake in the Amolatar District and Apac District in Uganda. It is near or linked to Lake Kyoga.</obo:IAO_0000115>
        <oboInOwl:hasOBONamespace>GAZ</oboInOwl:hasOBONamespace>
        <oboInOwl:id>GAZ:00058793</oboInOwl:id>
        <rdfs:label>Lake Kwania</rdfs:label>
    </owl:NamedIndividual>
    


    <!-- http://purl.obolibrary.org/obo/GAZ_00058802 -->

    <owl:NamedIndividual rdf:about="http://purl.obolibrary.org/obo/GAZ_00058802">
        <obo:RO_0001025 rdf:resource="http://purl.obolibrary.org/obo/GAZ_00000007"/>
        <obo:RO_0001025 rdf:resource="http://purl.obolibrary.org/obo/GAZ_00136138"/>
        <obo:IAO_0000115>The world&apos;s largest unbroken, unflooded volcanic caldera. The Crater, which formed when a giant volcano exploded and collapsed on itself some two to three million years ago, is 610m deep and the floor is 260 km2.</obo:IAO_0000115>
        <oboInOwl:hasOBONamespace>GAZ</oboInOwl:hasOBONamespace>
        <oboInOwl:id>GAZ:00058802</oboInOwl:id>
        <rdfs:label>Ngorongoro Crater</rdfs:label>
    </owl:NamedIndividual>
    


    <!-- http://purl.obolibrary.org/obo/GAZ_00058803 -->

    <owl:NamedIndividual rdf:about="http://purl.obolibrary.org/obo/GAZ_00058803">
        <obo:RO_0001025 rdf:resource="http://purl.obolibrary.org/obo/GAZ_00000007"/>
        <obo:IAO_0000115>A steep-sided ravine in the Great Rift Valley, which stretches along eastern Africa. Olduvai is in the eastern Serengeti Plains in northern Tanzania and is about 30 miles long.</obo:IAO_0000115>
        <oboInOwl:hasOBONamespace>GAZ</oboInOwl:hasOBONamespace>
        <oboInOwl:id>GAZ:00058803</oboInOwl:id>
        <rdfs:label>Olduvai Gorge</rdfs:label>
    </owl:NamedIndividual>
    


    <!-- http://purl.obolibrary.org/obo/GAZ_00058820 -->

    <owl:NamedIndividual rdf:about="http://purl.obolibrary.org/obo/GAZ_00058820">
        <obo:RO_0001025 rdf:resource="http://purl.obolibrary.org/obo/GAZ_00053526"/>
        <obo:IAO_0000115>A lake in Rwanda. Located on the southern slopes of Mount Muhabura.</obo:IAO_0000115>
        <oboInOwl:hasOBONamespace>GAZ</oboInOwl:hasOBONamespace>
        <oboInOwl:id>GAZ:00058820</oboInOwl:id>
        <rdfs:label>Lake Burera</rdfs:label>
    </owl:NamedIndividual>
    


    <!-- http://purl.obolibrary.org/obo/GAZ_00058835 -->

    <owl:NamedIndividual rdf:about="http://purl.obolibrary.org/obo/GAZ_00058835">
        <obo:RO_0001025 rdf:resource="http://purl.obolibrary.org/obo/GAZ_00058836"/>
        <obo:IAO_0000115>An oxbow lake in Kenya, at the base of the Kerio valley. The lake is 1 km2 in size. It was formed in year 1961 as a result of the Kerio River changing its course, therefore forming an oxbow lake.</obo:IAO_0000115>
        <oboInOwl:hasOBONamespace>GAZ</oboInOwl:hasOBONamespace>
        <oboInOwl:id>GAZ:00058835</oboInOwl:id>
        <rdfs:label>Lake Kamnarok</rdfs:label>
    </owl:NamedIndividual>
    


    <!-- http://purl.obolibrary.org/obo/GAZ_00058836 -->

    <owl:NamedIndividual rdf:about="http://purl.obolibrary.org/obo/GAZ_00058836">
        <obo:RO_0001025 rdf:resource="http://purl.obolibrary.org/obo/GAZ_00000007"/>
        <obo:IAO_0000115>A valley that lies between the Tugen Hills and the Elgeyo escarpment at an elevation of 1,000 m. in the Great Rift Valley in Kenya.</obo:IAO_0000115>
        <oboInOwl:hasOBONamespace>GAZ</oboInOwl:hasOBONamespace>
        <oboInOwl:id>GAZ:00058836</oboInOwl:id>
        <rdfs:label>Kerio River Valley</rdfs:label>
    </owl:NamedIndividual>
    


    <!-- http://purl.obolibrary.org/obo/GAZ_00058840 -->

    <owl:NamedIndividual rdf:about="http://purl.obolibrary.org/obo/GAZ_00058840">
        <obo:IAO_0000115>A reservoir in south-central Ethiopia. It was created by the construction of the Koka Dam across the Awash River. It is Located in the Misraq Shewa Zone of the Oromia Region. Constructed 1960.</obo:IAO_0000115>
        <oboInOwl:hasOBONamespace>GAZ</oboInOwl:hasOBONamespace>
        <oboInOwl:id>GAZ:00058840</oboInOwl:id>
        <rdfs:label>Koka Reservoir</rdfs:label>
    </owl:NamedIndividual>
    


    <!-- http://purl.obolibrary.org/obo/GAZ_00076405 -->

    <owl:NamedIndividual rdf:about="http://purl.obolibrary.org/obo/GAZ_00076405">
        <obo:RO_0001025 rdf:resource="http://purl.obolibrary.org/obo/GAZ_00000007"/>
        <obo:IAO_0000115>A national park that lies south of Lake Naivasha in Kenya, north west of Nairobi. It includes the Fischer&apos;s Tower and Central Tower columns and Hell&apos;s Gate Gorge. The national park is also home to three geothermal power stations at Olkaria.</obo:IAO_0000115>
        <oboInOwl:hasOBONamespace>GAZ</oboInOwl:hasOBONamespace>
        <oboInOwl:id>GAZ:00076405</oboInOwl:id>
        <rdfs:label>Hell&apos;s Gate National Park</rdfs:label>
    </owl:NamedIndividual>
    


    <!-- http://purl.obolibrary.org/obo/GAZ_00076409 -->

    <owl:NamedIndividual rdf:about="http://purl.obolibrary.org/obo/GAZ_00076409">
        <obo:IAO_0000115>A national park that straddles the Western border of Kenya and Uganda. Located in the Trans-Nzoia District of Rift Valley Province, The park was gazetted in 1968. Mt. Elgon National Park is located on the North Eastern side of the mountain.</obo:IAO_0000115>
        <oboInOwl:hasOBONamespace>GAZ</oboInOwl:hasOBONamespace>
        <oboInOwl:id>GAZ:00076409</oboInOwl:id>
        <rdfs:label>Mount Elgon National Park</rdfs:label>
    </owl:NamedIndividual>
    


    <!-- http://purl.obolibrary.org/obo/GAZ_00076707 -->

    <owl:NamedIndividual rdf:about="http://purl.obolibrary.org/obo/GAZ_00076707">
        <obo:RO_0001025 rdf:resource="http://purl.obolibrary.org/obo/GAZ_00076708"/>
        <obo:IAO_0000115>A national park in Tanzania.</obo:IAO_0000115>
        <oboInOwl:hasOBONamespace>GAZ</oboInOwl:hasOBONamespace>
        <oboInOwl:id>GAZ:00076707</oboInOwl:id>
        <rdfs:label>Rubondo Island National Park</rdfs:label>
    </owl:NamedIndividual>
    


    <!-- http://purl.obolibrary.org/obo/GAZ_00076708 -->

    <owl:NamedIndividual rdf:about="http://purl.obolibrary.org/obo/GAZ_00076708">
        <obo:RO_0001025 rdf:resource="http://purl.obolibrary.org/obo/GAZ_00015452"/>
        <obo:IAO_0000115>An island in the SW of Lake Victoria.</obo:IAO_0000115>
        <oboInOwl:hasOBONamespace>GAZ</oboInOwl:hasOBONamespace>
        <oboInOwl:id>GAZ:00076708</oboInOwl:id>
        <rdfs:label>Rubondo Island</rdfs:label>
    </owl:NamedIndividual>
    


    <!-- http://purl.obolibrary.org/obo/GAZ_00076715 -->

    <owl:NamedIndividual rdf:about="http://purl.obolibrary.org/obo/GAZ_00076715">
        <obo:RO_0001025 rdf:resource="http://purl.obolibrary.org/obo/GAZ_00000007"/>
        <obo:IAO_0000115>A protected area in Tanzania.</obo:IAO_0000115>
        <oboInOwl:hasOBONamespace>GAZ</oboInOwl:hasOBONamespace>
        <oboInOwl:id>GAZ:00076715</oboInOwl:id>
        <rdfs:label>Uwanda Game Reserve</rdfs:label>
    </owl:NamedIndividual>
    


    <!-- http://purl.obolibrary.org/obo/GAZ_00076726 -->

    <owl:NamedIndividual rdf:about="http://purl.obolibrary.org/obo/GAZ_00076726">
        <obo:IAO_0000115>A national park located in southwestern Uganda in East Africa. The park is part of the Bwindi Impenetrable Forest, and is situated along the Democratic Republic of Congo border next to the Virunga National Park and on the edge of the western Rift Valley. A World Heritage Site.</obo:IAO_0000115>
        <oboInOwl:hasOBONamespace>GAZ</oboInOwl:hasOBONamespace>
        <oboInOwl:id>GAZ:00076726</oboInOwl:id>
        <rdfs:label>Bwindi Impenetrable National Park</rdfs:label>
    </owl:NamedIndividual>
    


    <!-- http://purl.obolibrary.org/obo/GAZ_00076728 -->

    <owl:NamedIndividual rdf:about="http://purl.obolibrary.org/obo/GAZ_00076728">
        <obo:IAO_0000115>A 1436 km2 national park in Karamoja region in northwest Uganda. Kidepo is rugged savannah, dominated by the 2750 m Mount Morungole and transected by the Rivers Kidepo and Narus.</obo:IAO_0000115>
        <oboInOwl:hasOBONamespace>GAZ</oboInOwl:hasOBONamespace>
        <oboInOwl:id>GAZ:00076728</oboInOwl:id>
        <rdfs:label>Kidepo Valley National Park</rdfs:label>
    </owl:NamedIndividual>
    


    <!-- http://purl.obolibrary.org/obo/GAZ_00076729 -->

    <owl:NamedIndividual rdf:about="http://purl.obolibrary.org/obo/GAZ_00076729">
        <obo:RO_0001025 rdf:resource="http://purl.obolibrary.org/obo/GAZ_00009917"/>
        <obo:IAO_0000115>A national park located in western Uganda.</obo:IAO_0000115>
        <oboInOwl:hasOBONamespace>GAZ</oboInOwl:hasOBONamespace>
        <oboInOwl:id>GAZ:00076729</oboInOwl:id>
        <rdfs:label>Lake Mburo National Park</rdfs:label>
    </owl:NamedIndividual>
    


    <!-- http://purl.obolibrary.org/obo/GAZ_00076730 -->

    <owl:NamedIndividual rdf:about="http://purl.obolibrary.org/obo/GAZ_00076730">
        <obo:RO_0001025 rdf:resource="http://purl.obolibrary.org/obo/GAZ_00009915"/>
        <obo:IAO_0000115>A national park that lies in north western Uganda, spreading inland from the shore of Lake Albert around the Victoria Nile.</obo:IAO_0000115>
        <oboInOwl:hasOBONamespace>GAZ</oboInOwl:hasOBONamespace>
        <oboInOwl:id>GAZ:00076730</oboInOwl:id>
        <rdfs:label>Murchison Falls National Park</rdfs:label>
    </owl:NamedIndividual>
    


    <!-- http://purl.obolibrary.org/obo/GAZ_00076731 -->

    <owl:NamedIndividual rdf:about="http://purl.obolibrary.org/obo/GAZ_00076731">
        <obo:RO_0001025 rdf:resource="http://purl.obolibrary.org/obo/GAZ_00015394"/>
        <obo:IAO_0000115>A national park that ies in the west of the nation and occupies 5,000 km2 from Lake George to Lake Edward around the Kazinga Channel connecting them. The national park includes the Maramagambo Forest and borders the Kigezi and Kyambura Game Reserves, Kibale National Park, and the Virunga National Park in the Democratic Republic of Congo. Kasese lies on the north western edge of the park.</obo:IAO_0000115>
        <oboInOwl:hasOBONamespace>GAZ</oboInOwl:hasOBONamespace>
        <oboInOwl:id>GAZ:00076731</oboInOwl:id>
        <rdfs:label>Queen Elizabeth National Park</rdfs:label>
    </owl:NamedIndividual>
    


    <!-- http://purl.obolibrary.org/obo/GAZ_00076733 -->

    <owl:NamedIndividual rdf:about="http://purl.obolibrary.org/obo/GAZ_00076733">
        <obo:IAO_0000115>A national park and UNESCO World Heritage Site located in the Ruwenzori Mountains of Uganda.</obo:IAO_0000115>
        <oboInOwl:hasOBONamespace>GAZ</oboInOwl:hasOBONamespace>
        <oboInOwl:id>GAZ:00076733</oboInOwl:id>
        <rdfs:label>Rwenzori Mountains National Park</rdfs:label>
    </owl:NamedIndividual>
    


    <!-- http://purl.obolibrary.org/obo/GAZ_00076734 -->

    <owl:NamedIndividual rdf:about="http://purl.obolibrary.org/obo/GAZ_00076734">
        <obo:RO_0001025 rdf:resource="http://purl.obolibrary.org/obo/GAZ_00015558"/>
        <obo:IAO_0000115>A national park located in Bwamba County, a remote part of the Bundibugyo District in western Uganda. Established 1993-10.</obo:IAO_0000115>
        <oboInOwl:hasOBONamespace>GAZ</oboInOwl:hasOBONamespace>
        <oboInOwl:id>GAZ:00076734</oboInOwl:id>
        <rdfs:label>Semuliki National Park</rdfs:label>
    </owl:NamedIndividual>
    


    <!-- http://purl.obolibrary.org/obo/GAZ_00123116 -->

    <owl:NamedIndividual rdf:about="http://purl.obolibrary.org/obo/GAZ_00123116">
        <obo:RO_0001025 rdf:resource="http://purl.obolibrary.org/obo/GAZ_00053526"/>
        <obo:IAO_0000115>A lake in Rwanda. It lies just to the south of Lake Bulera, separated from it by a spine of hills.</obo:IAO_0000115>
        <oboInOwl:hasOBONamespace>GAZ</oboInOwl:hasOBONamespace>
        <oboInOwl:id>GAZ:00123116</oboInOwl:id>
        <rdfs:label>Lake Ruhondo</rdfs:label>
    </owl:NamedIndividual>
    


    <!-- http://purl.obolibrary.org/obo/GAZ_00124218 -->

    <owl:NamedIndividual rdf:about="http://purl.obolibrary.org/obo/GAZ_00124218">
        <obo:RO_0001025 rdf:resource="http://purl.obolibrary.org/obo/GAZ_00000007"/>
        <obo:IAO_0000115>A series of hills in Baringo District, Kenya.</obo:IAO_0000115>
        <oboInOwl:hasOBONamespace>GAZ</oboInOwl:hasOBONamespace>
        <oboInOwl:id>GAZ:00124218</oboInOwl:id>
        <rdfs:label>Tugen Hills</rdfs:label>
    </owl:NamedIndividual>
    


    <!-- http://purl.obolibrary.org/obo/GAZ_00124306 -->

    <owl:NamedIndividual rdf:about="http://purl.obolibrary.org/obo/GAZ_00124306">
        <obo:RO_0001025 rdf:resource="http://purl.obolibrary.org/obo/GAZ_00000007"/>
        <obo:IAO_0000115>A steep natural cliff approximately 3,000 m high, running along the western edge of the Great Rift Valley in Kenya.</obo:IAO_0000115>
        <oboInOwl:hasOBONamespace>GAZ</oboInOwl:hasOBONamespace>
        <oboInOwl:id>GAZ:00124306</oboInOwl:id>
        <rdfs:label>Mau Escarpment</rdfs:label>
    </owl:NamedIndividual>
    


    <!-- http://purl.obolibrary.org/obo/GAZ_00124307 -->

    <owl:NamedIndividual rdf:about="http://purl.obolibrary.org/obo/GAZ_00124307">
        <obo:RO_0001025 rdf:resource="http://purl.obolibrary.org/obo/GAZ_00124306"/>
        <obo:IAO_0000115>A forest complex in the Rift Valley of Kenya. It is the largest indigenous montane forest in East Africa. The Mau Forest complex has an area of 273300 ha.</obo:IAO_0000115>
        <oboInOwl:hasOBONamespace>GAZ</oboInOwl:hasOBONamespace>
        <oboInOwl:id>GAZ:00124307</oboInOwl:id>
        <rdfs:label>Mau Forest</rdfs:label>
    </owl:NamedIndividual>
    


    <!-- http://purl.obolibrary.org/obo/GAZ_00124567 -->

    <owl:NamedIndividual rdf:about="http://purl.obolibrary.org/obo/GAZ_00124567">
        <obo:RO_0001025 rdf:resource="http://purl.obolibrary.org/obo/GAZ_00015452"/>
        <oboInOwl:hasOBONamespace>GAZ</oboInOwl:hasOBONamespace>
        <oboInOwl:id>GAZ:00124567</oboInOwl:id>
        <rdfs:label>Napoleon Gulf</rdfs:label>
    </owl:NamedIndividual>
    


    <!-- http://purl.obolibrary.org/obo/GAZ_00124568 -->

    <owl:NamedIndividual rdf:about="http://purl.obolibrary.org/obo/GAZ_00124568">
        <obo:RO_0001025 rdf:resource="http://purl.obolibrary.org/obo/GAZ_00015453"/>
        <obo:IAO_0000115>The largest of the Buvuma Islands.</obo:IAO_0000115>
        <oboInOwl:hasOBONamespace>GAZ</oboInOwl:hasOBONamespace>
        <oboInOwl:id>GAZ:00124568</oboInOwl:id>
        <rdfs:label>Buvuma Island</rdfs:label>
    </owl:NamedIndividual>
    


    <!-- http://purl.obolibrary.org/obo/GAZ_00124569 -->

    <owl:NamedIndividual rdf:about="http://purl.obolibrary.org/obo/GAZ_00124569">
        <obo:RO_0001025 rdf:resource="http://purl.obolibrary.org/obo/GAZ_00015452"/>
        <obo:RO_0001025 rdf:resource="http://purl.obolibrary.org/obo/GAZ_00015453"/>
        <obo:IAO_0000115>One of the Buvuma Islands.</obo:IAO_0000115>
        <oboInOwl:hasOBONamespace>GAZ</oboInOwl:hasOBONamespace>
        <oboInOwl:id>GAZ:00124569</oboInOwl:id>
        <rdfs:label>Bugaia Island</rdfs:label>
    </owl:NamedIndividual>
    


    <!-- http://purl.obolibrary.org/obo/GAZ_00124570 -->

    <owl:NamedIndividual rdf:about="http://purl.obolibrary.org/obo/GAZ_00124570">
        <obo:RO_0001025 rdf:resource="http://purl.obolibrary.org/obo/GAZ_00015452"/>
        <obo:RO_0001025 rdf:resource="http://purl.obolibrary.org/obo/GAZ_00015453"/>
        <obo:IAO_0000115>One of the Buvuma Islands.</obo:IAO_0000115>
        <oboInOwl:hasOBONamespace>GAZ</oboInOwl:hasOBONamespace>
        <oboInOwl:id>GAZ:00124570</oboInOwl:id>
        <rdfs:label>Lingira Island</rdfs:label>
    </owl:NamedIndividual>
    


    <!-- http://purl.obolibrary.org/obo/GAZ_00124571 -->

    <owl:NamedIndividual rdf:about="http://purl.obolibrary.org/obo/GAZ_00124571">
        <obo:RO_0001025 rdf:resource="http://purl.obolibrary.org/obo/GAZ_00015452"/>
        <obo:RO_0001025 rdf:resource="http://purl.obolibrary.org/obo/GAZ_00015453"/>
        <obo:IAO_0000115>One of the Buvuma Islands.</obo:IAO_0000115>
        <oboInOwl:hasOBONamespace>GAZ</oboInOwl:hasOBONamespace>
        <oboInOwl:id>GAZ:00124571</oboInOwl:id>
        <rdfs:label>Namiti Island</rdfs:label>
    </owl:NamedIndividual>
    


    <!-- http://purl.obolibrary.org/obo/GAZ_00136138 -->

    <owl:NamedIndividual rdf:about="http://purl.obolibrary.org/obo/GAZ_00136138">
        <obo:RO_0001025 rdf:resource="http://purl.obolibrary.org/obo/GAZ_00000007"/>
        <obo:IAO_0000115>A region along the East African Rift in Tanzania, located in a spreading zone at the intersection of branches of the African and Somali tectonic plates.</obo:IAO_0000115>
        <oboInOwl:hasOBONamespace>GAZ</oboInOwl:hasOBONamespace>
        <oboInOwl:id>GAZ:00136138</oboInOwl:id>
        <rdfs:label>Crater Highlands</rdfs:label>
    </owl:NamedIndividual>
    


    <!-- http://purl.obolibrary.org/obo/GAZ_00136139 -->

    <owl:NamedIndividual rdf:about="http://purl.obolibrary.org/obo/GAZ_00136139">
        <obo:RO_0001025 rdf:resource="http://purl.obolibrary.org/obo/GAZ_00136138"/>
        <oboInOwl:hasOBONamespace>GAZ</oboInOwl:hasOBONamespace>
        <oboInOwl:id>GAZ:00136139</oboInOwl:id>
        <rdfs:label>Ela Naibori Crater</rdfs:label>
    </owl:NamedIndividual>
    


    <!-- http://purl.obolibrary.org/obo/GAZ_00136140 -->

    <owl:NamedIndividual rdf:about="http://purl.obolibrary.org/obo/GAZ_00136140">
        <obo:RO_0001025 rdf:resource="http://purl.obolibrary.org/obo/GAZ_00136138"/>
        <obo:IAO_0000115>A volcano located in Tanzania in the Crater Highlands region. It is at the southeastern edge of Lake Natron in Africa&apos;s Great Rift Valley.</obo:IAO_0000115>
        <oboInOwl:hasOBONamespace>GAZ</oboInOwl:hasOBONamespace>
        <oboInOwl:id>GAZ:00136140</oboInOwl:id>
        <rdfs:label>Gelai Volcano</rdfs:label>
    </owl:NamedIndividual>
    


    <!-- http://purl.obolibrary.org/obo/GAZ_00136141 -->

    <owl:NamedIndividual rdf:about="http://purl.obolibrary.org/obo/GAZ_00136141">
        <obo:RO_0001025 rdf:resource="http://purl.obolibrary.org/obo/GAZ_00136138"/>
        <oboInOwl:hasOBONamespace>GAZ</oboInOwl:hasOBONamespace>
        <oboInOwl:id>GAZ:00136141</oboInOwl:id>
        <rdfs:label>Meto Hills</rdfs:label>
    </owl:NamedIndividual>
    


    <!-- http://purl.obolibrary.org/obo/GAZ_00144024 -->

    <owl:NamedIndividual rdf:about="http://purl.obolibrary.org/obo/GAZ_00144024">
        <obo:RO_0001025 rdf:resource="http://purl.obolibrary.org/obo/GAZ_00144031"/>
        <obo:IAO_0000115>A glacier on Mount Speke.</obo:IAO_0000115>
        <oboInOwl:hasOBONamespace>GAZ</oboInOwl:hasOBONamespace>
        <oboInOwl:id>GAZ:00144024</oboInOwl:id>
        <rdfs:label>Speke Glacier</rdfs:label>
    </owl:NamedIndividual>
    


    <!-- http://purl.obolibrary.org/obo/GAZ_00144028 -->

    <owl:NamedIndividual rdf:about="http://purl.obolibrary.org/obo/GAZ_00144028">
        <obo:RO_0001025 rdf:resource="http://purl.obolibrary.org/obo/GAZ_00076733"/>
        <oboInOwl:hasOBONamespace>GAZ</oboInOwl:hasOBONamespace>
        <oboInOwl:id>GAZ:00144028</oboInOwl:id>
        <rdfs:label>Mount Emin</rdfs:label>
    </owl:NamedIndividual>
    


    <!-- http://purl.obolibrary.org/obo/GAZ_00144029 -->

    <owl:NamedIndividual rdf:about="http://purl.obolibrary.org/obo/GAZ_00144029">
        <obo:RO_0001025 rdf:resource="http://purl.obolibrary.org/obo/GAZ_00076733"/>
        <oboInOwl:hasOBONamespace>GAZ</oboInOwl:hasOBONamespace>
        <oboInOwl:id>GAZ:00144029</oboInOwl:id>
        <rdfs:label>Mount Stanley</rdfs:label>
    </owl:NamedIndividual>
    


    <!-- http://purl.obolibrary.org/obo/GAZ_00144030 -->

    <owl:NamedIndividual rdf:about="http://purl.obolibrary.org/obo/GAZ_00144030">
        <obo:RO_0001025 rdf:resource="http://purl.obolibrary.org/obo/GAZ_00076733"/>
        <oboInOwl:hasOBONamespace>GAZ</oboInOwl:hasOBONamespace>
        <oboInOwl:id>GAZ:00144030</oboInOwl:id>
        <rdfs:label>Mount Gessi</rdfs:label>
    </owl:NamedIndividual>
    


    <!-- http://purl.obolibrary.org/obo/GAZ_00144031 -->

    <owl:NamedIndividual rdf:about="http://purl.obolibrary.org/obo/GAZ_00144031">
        <obo:RO_0001025 rdf:resource="http://purl.obolibrary.org/obo/GAZ_00076733"/>
        <oboInOwl:hasOBONamespace>GAZ</oboInOwl:hasOBONamespace>
        <oboInOwl:id>GAZ:00144031</oboInOwl:id>
        <rdfs:label>Mount Speke</rdfs:label>
    </owl:NamedIndividual>
    


    <!-- http://purl.obolibrary.org/obo/GAZ_00144032 -->

    <owl:NamedIndividual rdf:about="http://purl.obolibrary.org/obo/GAZ_00144032">
        <obo:RO_0001025 rdf:resource="http://purl.obolibrary.org/obo/GAZ_00076733"/>
        <oboInOwl:hasOBONamespace>GAZ</oboInOwl:hasOBONamespace>
        <oboInOwl:id>GAZ:00144032</oboInOwl:id>
        <rdfs:label>Mount Luigi di Savoia</rdfs:label>
    </owl:NamedIndividual>
    


    <!-- http://purl.obolibrary.org/obo/GAZ_00144033 -->

    <owl:NamedIndividual rdf:about="http://purl.obolibrary.org/obo/GAZ_00144033">
        <obo:RO_0001025 rdf:resource="http://purl.obolibrary.org/obo/GAZ_00076733"/>
        <oboInOwl:hasOBONamespace>GAZ</oboInOwl:hasOBONamespace>
        <oboInOwl:id>GAZ:00144033</oboInOwl:id>
        <rdfs:label>Mount Baker</rdfs:label>
    </owl:NamedIndividual>
    


    <!-- http://purl.obolibrary.org/obo/GAZ_00144034 -->

    <owl:NamedIndividual rdf:about="http://purl.obolibrary.org/obo/GAZ_00144034">
        <obo:RO_0001025 rdf:resource="http://purl.obolibrary.org/obo/GAZ_00144032"/>
        <obo:IAO_0000115>A former glacier on Mount Luigi di Savoia, disappeared by 1906.</obo:IAO_0000115>
        <oboInOwl:hasOBONamespace>GAZ</oboInOwl:hasOBONamespace>
        <oboInOwl:id>GAZ:00144034</oboInOwl:id>
        <rdfs:label>Stairs Glacier</rdfs:label>
    </owl:NamedIndividual>
    


    <!-- http://purl.obolibrary.org/obo/GAZ_00144035 -->

    <owl:NamedIndividual rdf:about="http://purl.obolibrary.org/obo/GAZ_00144035">
        <obo:RO_0001025 rdf:resource="http://purl.obolibrary.org/obo/GAZ_00144032"/>
        <obo:IAO_0000115>A former glacier on Mount Luigi di Savoia, disappeared by 1906.</obo:IAO_0000115>
        <oboInOwl:hasOBONamespace>GAZ</oboInOwl:hasOBONamespace>
        <oboInOwl:id>GAZ:00144035</oboInOwl:id>
        <rdfs:label>Sella Galcier</rdfs:label>
    </owl:NamedIndividual>
    


    <!-- http://purl.obolibrary.org/obo/GAZ_00144036 -->

    <owl:NamedIndividual rdf:about="http://purl.obolibrary.org/obo/GAZ_00144036">
        <obo:RO_0001025 rdf:resource="http://purl.obolibrary.org/obo/GAZ_00144032"/>
        <obo:IAO_0000115>A glacier on Mount Luigi di Savoia.</obo:IAO_0000115>
        <oboInOwl:hasOBONamespace>GAZ</oboInOwl:hasOBONamespace>
        <oboInOwl:id>GAZ:00144036</oboInOwl:id>
        <rdfs:label>Thomson Glacier</rdfs:label>
    </owl:NamedIndividual>
    


    <!-- http://purl.obolibrary.org/obo/GAZ_00144037 -->

    <owl:NamedIndividual rdf:about="http://purl.obolibrary.org/obo/GAZ_00144037">
        <obo:RO_0001025 rdf:resource="http://purl.obolibrary.org/obo/GAZ_00144028"/>
        <obo:IAO_0000115>A glacier on Mount Emin.</obo:IAO_0000115>
        <oboInOwl:hasOBONamespace>GAZ</oboInOwl:hasOBONamespace>
        <oboInOwl:id>GAZ:00144037</oboInOwl:id>
        <rdfs:label>Emin Glacier</rdfs:label>
    </owl:NamedIndividual>
    


    <!-- http://purl.obolibrary.org/obo/GAZ_00144038 -->

    <owl:NamedIndividual rdf:about="http://purl.obolibrary.org/obo/GAZ_00144038">
        <obo:RO_0001025 rdf:resource="http://purl.obolibrary.org/obo/GAZ_00144028"/>
        <obo:IAO_0000115>A glacier on Mount Emin.</obo:IAO_0000115>
        <oboInOwl:hasOBONamespace>GAZ</oboInOwl:hasOBONamespace>
        <oboInOwl:id>GAZ:00144038</oboInOwl:id>
        <rdfs:label>Kraepelin Glacier</rdfs:label>
    </owl:NamedIndividual>
    


    <!-- http://purl.obolibrary.org/obo/GAZ_00144039 -->

    <owl:NamedIndividual rdf:about="http://purl.obolibrary.org/obo/GAZ_00144039">
        <obo:RO_0001025 rdf:resource="http://purl.obolibrary.org/obo/GAZ_00144028"/>
        <obo:IAO_0000115>A former glacier on Mount Emin, disappeared by 1906.</obo:IAO_0000115>
        <oboInOwl:hasOBONamespace>GAZ</oboInOwl:hasOBONamespace>
        <oboInOwl:id>GAZ:00144039</oboInOwl:id>
        <rdfs:label>Umberto Glacier</rdfs:label>
    </owl:NamedIndividual>
    


    <!-- http://purl.obolibrary.org/obo/GAZ_00144040 -->

    <owl:NamedIndividual rdf:about="http://purl.obolibrary.org/obo/GAZ_00144040">
        <obo:RO_0001025 rdf:resource="http://purl.obolibrary.org/obo/GAZ_00144033"/>
        <obo:IAO_0000115>A glacier on Mount Baker.</obo:IAO_0000115>
        <oboInOwl:hasOBONamespace>GAZ</oboInOwl:hasOBONamespace>
        <oboInOwl:id>GAZ:00144040</oboInOwl:id>
        <rdfs:label>Moore Glacier</rdfs:label>
    </owl:NamedIndividual>
    


    <!-- http://purl.obolibrary.org/obo/GAZ_00144041 -->

    <owl:NamedIndividual rdf:about="http://purl.obolibrary.org/obo/GAZ_00144041">
        <obo:RO_0001025 rdf:resource="http://purl.obolibrary.org/obo/GAZ_00144033"/>
        <obo:IAO_0000115>A glacier on Mount Baker.</obo:IAO_0000115>
        <oboInOwl:hasOBONamespace>GAZ</oboInOwl:hasOBONamespace>
        <oboInOwl:id>GAZ:00144041</oboInOwl:id>
        <rdfs:label>Edward 2 Glacier</rdfs:label>
    </owl:NamedIndividual>
    


    <!-- http://purl.obolibrary.org/obo/GAZ_00144042 -->

    <owl:NamedIndividual rdf:about="http://purl.obolibrary.org/obo/GAZ_00144042">
        <obo:RO_0001025 rdf:resource="http://purl.obolibrary.org/obo/GAZ_00144033"/>
        <obo:IAO_0000115>A former glacier on Mount Baker, disappeared after 1943.</obo:IAO_0000115>
        <oboInOwl:hasOBONamespace>GAZ</oboInOwl:hasOBONamespace>
        <oboInOwl:id>GAZ:00144042</oboInOwl:id>
        <rdfs:label>Semperb Glacier</rdfs:label>
    </owl:NamedIndividual>
    


    <!-- http://purl.obolibrary.org/obo/GAZ_00144043 -->

    <owl:NamedIndividual rdf:about="http://purl.obolibrary.org/obo/GAZ_00144043">
        <obo:RO_0001025 rdf:resource="http://purl.obolibrary.org/obo/GAZ_00144033"/>
        <obo:IAO_0000115>A glacier on Mount Baker.</obo:IAO_0000115>
        <oboInOwl:hasOBONamespace>GAZ</oboInOwl:hasOBONamespace>
        <oboInOwl:id>GAZ:00144043</oboInOwl:id>
        <rdfs:label>Wollaston Glacier</rdfs:label>
    </owl:NamedIndividual>
    


    <!-- http://purl.obolibrary.org/obo/GAZ_00144044 -->

    <owl:NamedIndividual rdf:about="http://purl.obolibrary.org/obo/GAZ_00144044">
        <obo:RO_0001025 rdf:resource="http://purl.obolibrary.org/obo/GAZ_00144033"/>
        <obo:IAO_0000115>A glacier on Mount Baker.</obo:IAO_0000115>
        <oboInOwl:hasOBONamespace>GAZ</oboInOwl:hasOBONamespace>
        <oboInOwl:id>GAZ:00144044</oboInOwl:id>
        <rdfs:label>Edward 1 Glacier</rdfs:label>
    </owl:NamedIndividual>
    


    <!-- http://purl.obolibrary.org/obo/GAZ_00144045 -->

    <owl:NamedIndividual rdf:about="http://purl.obolibrary.org/obo/GAZ_00144045">
        <obo:RO_0001025 rdf:resource="http://purl.obolibrary.org/obo/GAZ_00144033"/>
        <obo:IAO_0000115>A glacier on Mount Baker.</obo:IAO_0000115>
        <oboInOwl:hasOBONamespace>GAZ</oboInOwl:hasOBONamespace>
        <oboInOwl:id>GAZ:00144045</oboInOwl:id>
        <rdfs:label>Y Glacier</rdfs:label>
    </owl:NamedIndividual>
    


    <!-- http://purl.obolibrary.org/obo/GAZ_00144046 -->

    <owl:NamedIndividual rdf:about="http://purl.obolibrary.org/obo/GAZ_00144046">
        <obo:RO_0001025 rdf:resource="http://purl.obolibrary.org/obo/GAZ_00144033"/>
        <obo:IAO_0000115>A glacier on Mount Baker.</obo:IAO_0000115>
        <oboInOwl:hasOBONamespace>GAZ</oboInOwl:hasOBONamespace>
        <oboInOwl:id>GAZ:00144046</oboInOwl:id>
        <rdfs:label>Edward 3 Glacier</rdfs:label>
    </owl:NamedIndividual>
    


    <!-- http://purl.obolibrary.org/obo/GAZ_00144047 -->

    <owl:NamedIndividual rdf:about="http://purl.obolibrary.org/obo/GAZ_00144047">
        <obo:RO_0001025 rdf:resource="http://purl.obolibrary.org/obo/GAZ_00144033"/>
        <obo:IAO_0000115>A glacier on Mount Baker.</obo:IAO_0000115>
        <oboInOwl:hasOBONamespace>GAZ</oboInOwl:hasOBONamespace>
        <oboInOwl:id>GAZ:00144047</oboInOwl:id>
        <rdfs:label>East Baker Glacier</rdfs:label>
    </owl:NamedIndividual>
    


    <!-- http://purl.obolibrary.org/obo/GAZ_00144048 -->

    <owl:NamedIndividual rdf:about="http://purl.obolibrary.org/obo/GAZ_00144048">
        <obo:RO_0001025 rdf:resource="http://purl.obolibrary.org/obo/GAZ_00144033"/>
        <obo:IAO_0000115>A glacier on Mount Baker.</obo:IAO_0000115>
        <oboInOwl:hasOBONamespace>GAZ</oboInOwl:hasOBONamespace>
        <oboInOwl:id>GAZ:00144048</oboInOwl:id>
        <rdfs:label>West Baker Glacier</rdfs:label>
    </owl:NamedIndividual>
    


    <!-- http://purl.obolibrary.org/obo/GAZ_00144049 -->

    <owl:NamedIndividual rdf:about="http://purl.obolibrary.org/obo/GAZ_00144049">
        <obo:RO_0001025 rdf:resource="http://purl.obolibrary.org/obo/GAZ_00144030"/>
        <obo:IAO_0000115>A glacier on Mount Gessi.</obo:IAO_0000115>
        <oboInOwl:hasOBONamespace>GAZ</oboInOwl:hasOBONamespace>
        <oboInOwl:id>GAZ:00144049</oboInOwl:id>
        <rdfs:label>Iolanda 1 Glacier</rdfs:label>
    </owl:NamedIndividual>
    


    <!-- http://purl.obolibrary.org/obo/GAZ_00144050 -->

    <owl:NamedIndividual rdf:about="http://purl.obolibrary.org/obo/GAZ_00144050">
        <obo:RO_0001025 rdf:resource="http://purl.obolibrary.org/obo/GAZ_00144030"/>
        <obo:IAO_0000115>A glacier on Mount Gessi.</obo:IAO_0000115>
        <oboInOwl:hasOBONamespace>GAZ</oboInOwl:hasOBONamespace>
        <oboInOwl:id>GAZ:00144050</oboInOwl:id>
        <rdfs:label>Iolanda 2 Glacier</rdfs:label>
    </owl:NamedIndividual>
    


    <!-- http://purl.obolibrary.org/obo/GAZ_00144051 -->

    <owl:NamedIndividual rdf:about="http://purl.obolibrary.org/obo/GAZ_00144051">
        <obo:RO_0001025 rdf:resource="http://purl.obolibrary.org/obo/GAZ_00144030"/>
        <obo:IAO_0000115>A glacier on Mount Gessi.</obo:IAO_0000115>
        <oboInOwl:hasOBONamespace>GAZ</oboInOwl:hasOBONamespace>
        <oboInOwl:id>GAZ:00144051</oboInOwl:id>
        <rdfs:label>Gessi 1 Glacier</rdfs:label>
    </owl:NamedIndividual>
    


    <!-- http://purl.obolibrary.org/obo/GAZ_00144052 -->

    <owl:NamedIndividual rdf:about="http://purl.obolibrary.org/obo/GAZ_00144052">
        <obo:RO_0001025 rdf:resource="http://purl.obolibrary.org/obo/GAZ_00144030"/>
        <obo:IAO_0000115>A glacier on Mount Gessi.</obo:IAO_0000115>
        <oboInOwl:hasOBONamespace>GAZ</oboInOwl:hasOBONamespace>
        <oboInOwl:id>GAZ:00144052</oboInOwl:id>
        <rdfs:label>Gessi 4 Glacier</rdfs:label>
    </owl:NamedIndividual>
    


    <!-- http://purl.obolibrary.org/obo/GAZ_00144053 -->

    <owl:NamedIndividual rdf:about="http://purl.obolibrary.org/obo/GAZ_00144053">
        <obo:RO_0001025 rdf:resource="http://purl.obolibrary.org/obo/GAZ_00144030"/>
        <obo:IAO_0000115>A glacier on Mount Gessi.</obo:IAO_0000115>
        <oboInOwl:hasOBONamespace>GAZ</oboInOwl:hasOBONamespace>
        <oboInOwl:id>GAZ:00144053</oboInOwl:id>
        <rdfs:label>Gessi 2 Glacier</rdfs:label>
    </owl:NamedIndividual>
    


    <!-- http://purl.obolibrary.org/obo/GAZ_00144054 -->

    <owl:NamedIndividual rdf:about="http://purl.obolibrary.org/obo/GAZ_00144054">
        <obo:RO_0001025 rdf:resource="http://purl.obolibrary.org/obo/GAZ_00144030"/>
        <obo:IAO_0000115>A glacier on Mount Gessi.</obo:IAO_0000115>
        <oboInOwl:hasOBONamespace>GAZ</oboInOwl:hasOBONamespace>
        <oboInOwl:id>GAZ:00144054</oboInOwl:id>
        <rdfs:label>Gessi 3 Glacier</rdfs:label>
    </owl:NamedIndividual>
    


    <!-- http://purl.obolibrary.org/obo/GAZ_00144055 -->

    <owl:NamedIndividual rdf:about="http://purl.obolibrary.org/obo/GAZ_00144055">
        <obo:RO_0001025 rdf:resource="http://purl.obolibrary.org/obo/GAZ_00144031"/>
        <obo:IAO_0000115>A glacier on Mount Speke.</obo:IAO_0000115>
        <oboInOwl:hasOBONamespace>GAZ</oboInOwl:hasOBONamespace>
        <oboInOwl:id>GAZ:00144055</oboInOwl:id>
        <rdfs:label>Johnston Glacier</rdfs:label>
    </owl:NamedIndividual>
    


    <!-- http://purl.obolibrary.org/obo/GAZ_00144056 -->

    <owl:NamedIndividual rdf:about="http://purl.obolibrary.org/obo/GAZ_00144056">
        <obo:RO_0001025 rdf:resource="http://purl.obolibrary.org/obo/GAZ_00144031"/>
        <obo:IAO_0000115>A glacier on Mount Speke.</obo:IAO_0000115>
        <oboInOwl:hasOBONamespace>GAZ</oboInOwl:hasOBONamespace>
        <oboInOwl:id>GAZ:00144056</oboInOwl:id>
        <rdfs:label>Vittorio Emanuele Glacier</rdfs:label>
    </owl:NamedIndividual>
    


    <!-- http://purl.obolibrary.org/obo/GAZ_00144057 -->

    <owl:NamedIndividual rdf:about="http://purl.obolibrary.org/obo/GAZ_00144057">
        <obo:RO_0001025 rdf:resource="http://purl.obolibrary.org/obo/GAZ_00144031"/>
        <obo:IAO_0000115>A glacier on Mount Speke.</obo:IAO_0000115>
        <oboInOwl:hasOBONamespace>GAZ</oboInOwl:hasOBONamespace>
        <oboInOwl:id>GAZ:00144057</oboInOwl:id>
        <rdfs:label>East Johnston Glacier</rdfs:label>
    </owl:NamedIndividual>
    


    <!-- http://purl.obolibrary.org/obo/GAZ_00144058 -->

    <owl:NamedIndividual rdf:about="http://purl.obolibrary.org/obo/GAZ_00144058">
        <obo:RO_0001025 rdf:resource="http://purl.obolibrary.org/obo/GAZ_00144031"/>
        <obo:IAO_0000115>A glacier on Mount Speke.</obo:IAO_0000115>
        <oboInOwl:hasOBONamespace>GAZ</oboInOwl:hasOBONamespace>
        <oboInOwl:id>GAZ:00144058</oboInOwl:id>
        <rdfs:label>Grant Glacier</rdfs:label>
    </owl:NamedIndividual>
    


    <!-- http://purl.obolibrary.org/obo/GAZ_00144059 -->

    <owl:NamedIndividual rdf:about="http://purl.obolibrary.org/obo/GAZ_00144059">
        <obo:RO_0001025 rdf:resource="http://purl.obolibrary.org/obo/GAZ_00144029"/>
        <obo:IAO_0000115>A glacier on Mount Stanley.</obo:IAO_0000115>
        <oboInOwl:hasOBONamespace>GAZ</oboInOwl:hasOBONamespace>
        <oboInOwl:id>GAZ:00144059</oboInOwl:id>
        <rdfs:label>Albert Glacier</rdfs:label>
    </owl:NamedIndividual>
    


    <!-- http://purl.obolibrary.org/obo/GAZ_00144060 -->

    <owl:NamedIndividual rdf:about="http://purl.obolibrary.org/obo/GAZ_00144060">
        <obo:RO_0001025 rdf:resource="http://purl.obolibrary.org/obo/GAZ_00144029"/>
        <obo:IAO_0000115>A glacier on Mount Stanley.</obo:IAO_0000115>
        <oboInOwl:hasOBONamespace>GAZ</oboInOwl:hasOBONamespace>
        <oboInOwl:id>GAZ:00144060</oboInOwl:id>
        <rdfs:label>North East Margherita Glacier</rdfs:label>
    </owl:NamedIndividual>
    


    <!-- http://purl.obolibrary.org/obo/GAZ_00144061 -->

    <owl:NamedIndividual rdf:about="http://purl.obolibrary.org/obo/GAZ_00144061">
        <obo:RO_0001025 rdf:resource="http://purl.obolibrary.org/obo/GAZ_00144029"/>
        <obo:IAO_0000115>A glacier on Mount Stanley.</obo:IAO_0000115>
        <oboInOwl:hasOBONamespace>GAZ</oboInOwl:hasOBONamespace>
        <oboInOwl:id>GAZ:00144061</oboInOwl:id>
        <rdfs:label>Coronation Glacier</rdfs:label>
    </owl:NamedIndividual>
    


    <!-- http://purl.obolibrary.org/obo/GAZ_00144062 -->

    <owl:NamedIndividual rdf:about="http://purl.obolibrary.org/obo/GAZ_00144062">
        <obo:RO_0001025 rdf:resource="http://purl.obolibrary.org/obo/GAZ_00144029"/>
        <obo:IAO_0000115>A glacier on Mount Stanley.</obo:IAO_0000115>
        <oboInOwl:hasOBONamespace>GAZ</oboInOwl:hasOBONamespace>
        <oboInOwl:id>GAZ:00144062</oboInOwl:id>
        <rdfs:label>West Savoia Glacier</rdfs:label>
    </owl:NamedIndividual>
    


    <!-- http://purl.obolibrary.org/obo/GAZ_00144063 -->

    <owl:NamedIndividual rdf:about="http://purl.obolibrary.org/obo/GAZ_00144063">
        <obo:RO_0001025 rdf:resource="http://purl.obolibrary.org/obo/GAZ_00144029"/>
        <obo:IAO_0000115>A glacier on Mount Stanley.</obo:IAO_0000115>
        <oboInOwl:hasOBONamespace>GAZ</oboInOwl:hasOBONamespace>
        <oboInOwl:id>GAZ:00144063</oboInOwl:id>
        <rdfs:label>West Stanley Glacier</rdfs:label>
    </owl:NamedIndividual>
    


    <!-- http://purl.obolibrary.org/obo/GAZ_00144064 -->

    <owl:NamedIndividual rdf:about="http://purl.obolibrary.org/obo/GAZ_00144064">
        <obo:RO_0001025 rdf:resource="http://purl.obolibrary.org/obo/GAZ_00144029"/>
        <obo:IAO_0000115>A glacier on Mount Stanley.</obo:IAO_0000115>
        <oboInOwl:hasOBONamespace>GAZ</oboInOwl:hasOBONamespace>
        <oboInOwl:id>GAZ:00144064</oboInOwl:id>
        <rdfs:label>Elena Glacier</rdfs:label>
    </owl:NamedIndividual>
    


    <!-- http://purl.obolibrary.org/obo/GAZ_00144065 -->

    <owl:NamedIndividual rdf:about="http://purl.obolibrary.org/obo/GAZ_00144065">
        <obo:RO_0001025 rdf:resource="http://purl.obolibrary.org/obo/GAZ_00144029"/>
        <obo:IAO_0000115>A glacier on Mount Stanley.</obo:IAO_0000115>
        <oboInOwl:hasOBONamespace>GAZ</oboInOwl:hasOBONamespace>
        <oboInOwl:id>GAZ:00144065</oboInOwl:id>
        <rdfs:label>Alexandra Glacier</rdfs:label>
    </owl:NamedIndividual>
    


    <!-- http://purl.obolibrary.org/obo/GAZ_00144066 -->

    <owl:NamedIndividual rdf:about="http://purl.obolibrary.org/obo/GAZ_00144066">
        <obo:RO_0001025 rdf:resource="http://purl.obolibrary.org/obo/GAZ_00144029"/>
        <obo:IAO_0000115>A glacier on Mount Stanley.</obo:IAO_0000115>
        <oboInOwl:hasOBONamespace>GAZ</oboInOwl:hasOBONamespace>
        <oboInOwl:id>GAZ:00144066</oboInOwl:id>
        <rdfs:label>Philip Glacier</rdfs:label>
    </owl:NamedIndividual>
    


    <!-- http://purl.obolibrary.org/obo/GAZ_00144067 -->

    <owl:NamedIndividual rdf:about="http://purl.obolibrary.org/obo/GAZ_00144067">
        <obo:RO_0001025 rdf:resource="http://purl.obolibrary.org/obo/GAZ_00144029"/>
        <obo:IAO_0000115>A glacier on Mount Stanley.</obo:IAO_0000115>
        <oboInOwl:hasOBONamespace>GAZ</oboInOwl:hasOBONamespace>
        <oboInOwl:id>GAZ:00144067</oboInOwl:id>
        <rdfs:label>Moebius Glacier</rdfs:label>
    </owl:NamedIndividual>
    


    <!-- http://purl.obolibrary.org/obo/GAZ_00144068 -->

    <owl:NamedIndividual rdf:about="http://purl.obolibrary.org/obo/GAZ_00144068">
        <obo:RO_0001025 rdf:resource="http://purl.obolibrary.org/obo/GAZ_00144029"/>
        <obo:IAO_0000115>A glacier on Mount Stanley.</obo:IAO_0000115>
        <oboInOwl:hasOBONamespace>GAZ</oboInOwl:hasOBONamespace>
        <oboInOwl:id>GAZ:00144068</oboInOwl:id>
        <rdfs:label>Elizabeth Glacier</rdfs:label>
    </owl:NamedIndividual>
    


    <!-- http://purl.obolibrary.org/obo/GAZ_00144069 -->

    <owl:NamedIndividual rdf:about="http://purl.obolibrary.org/obo/GAZ_00144069">
        <obo:RO_0001025 rdf:resource="http://purl.obolibrary.org/obo/GAZ_00144029"/>
        <obo:IAO_0000115>A glacier on Mount Stanley.</obo:IAO_0000115>
        <oboInOwl:hasOBONamespace>GAZ</oboInOwl:hasOBONamespace>
        <oboInOwl:id>GAZ:00144069</oboInOwl:id>
        <rdfs:label>West Elena Glacier</rdfs:label>
    </owl:NamedIndividual>
    


    <!-- http://purl.obolibrary.org/obo/GAZ_00144070 -->

    <owl:NamedIndividual rdf:about="http://purl.obolibrary.org/obo/GAZ_00144070">
        <obo:RO_0001025 rdf:resource="http://purl.obolibrary.org/obo/GAZ_00144029"/>
        <obo:IAO_0000115>A glacier on Mount Stanley.</obo:IAO_0000115>
        <oboInOwl:hasOBONamespace>GAZ</oboInOwl:hasOBONamespace>
        <oboInOwl:id>GAZ:00144070</oboInOwl:id>
        <rdfs:label>East Stanley Glacier</rdfs:label>
    </owl:NamedIndividual>
    


    <!-- http://purl.obolibrary.org/obo/GAZ_00144071 -->

    <owl:NamedIndividual rdf:about="http://purl.obolibrary.org/obo/GAZ_00144071">
        <obo:RO_0001025 rdf:resource="http://purl.obolibrary.org/obo/GAZ_00144029"/>
        <obo:IAO_0000115>A glacier on Mount Stanley.</obo:IAO_0000115>
        <oboInOwl:hasOBONamespace>GAZ</oboInOwl:hasOBONamespace>
        <oboInOwl:id>GAZ:00144071</oboInOwl:id>
        <rdfs:label>Savoia Glacier</rdfs:label>
    </owl:NamedIndividual>
    


    <!-- http://purl.obolibrary.org/obo/GAZ_00144072 -->

    <owl:NamedIndividual rdf:about="http://purl.obolibrary.org/obo/GAZ_00144072">
        <obo:RO_0001025 rdf:resource="http://purl.obolibrary.org/obo/GAZ_00144029"/>
        <obo:IAO_0000115>A glacier on Mount Stanley.</obo:IAO_0000115>
        <oboInOwl:hasOBONamespace>GAZ</oboInOwl:hasOBONamespace>
        <oboInOwl:id>GAZ:00144072</oboInOwl:id>
        <rdfs:label>Margherita Glacier</rdfs:label>
    </owl:NamedIndividual>
    


    <!-- http://purl.obolibrary.org/obo/GAZ_00146121 -->

    <owl:NamedIndividual rdf:about="http://purl.obolibrary.org/obo/GAZ_00146121">
        <obo:RO_0001025 rdf:resource="http://purl.obolibrary.org/obo/GAZ_00015546"/>
        <obo:IAO_0000115>Hot springs situated on the Kabale-Katuna road, 8 km out of Kabale, Uganda.</obo:IAO_0000115>
        <oboInOwl:hasOBONamespace>GAZ</oboInOwl:hasOBONamespace>
        <oboInOwl:id>GAZ:00146121</oboInOwl:id>
        <rdfs:label>Ihimba Hot Springs</rdfs:label>
    </owl:NamedIndividual>
    


    <!-- http://purl.obolibrary.org/obo/GAZ_00146122 -->

    <owl:NamedIndividual rdf:about="http://purl.obolibrary.org/obo/GAZ_00146122">
        <obo:RO_0001025 rdf:resource="http://purl.obolibrary.org/obo/GAZ_00015405"/>
        <obo:IAO_0000115>Hot springs in the Bushenyi District of western Uganda, and are located near the Kitagata trading centre.</obo:IAO_0000115>
        <oboInOwl:hasOBONamespace>GAZ</oboInOwl:hasOBONamespace>
        <oboInOwl:id>GAZ:00146122</oboInOwl:id>
        <rdfs:label>Kitagata Hot Springs</rdfs:label>
    </owl:NamedIndividual>
    


    <!-- http://purl.obolibrary.org/obo/GAZ_00176005 -->

    <owl:NamedIndividual rdf:about="http://purl.obolibrary.org/obo/GAZ_00176005">
        <obo:RO_0001025 rdf:resource="http://purl.obolibrary.org/obo/GAZ_00007862"/>
        <obo:IAO_0000115>An island in the northern Gulf of Aqaba off the shore of Egypt&apos;s eastern Sinai Peninsula.</obo:IAO_0000115>
        <oboInOwl:hasOBONamespace>GAZ</oboInOwl:hasOBONamespace>
        <oboInOwl:id>GAZ:00176005</oboInOwl:id>
        <rdfs:label>Pharaoh&apos;s Island</rdfs:label>
    </owl:NamedIndividual>
    


    <!-- http://purl.obolibrary.org/obo/GAZ_00193785 -->

    <owl:NamedIndividual rdf:about="http://purl.obolibrary.org/obo/GAZ_00193785">
        <obo:RO_0001025 rdf:resource="http://purl.obolibrary.org/obo/GAZ_00007520"/>
        <obo:IAO_0000115>A river. A tributary of the Jordan River.</obo:IAO_0000115>
        <oboInOwl:hasOBONamespace>GAZ</oboInOwl:hasOBONamespace>
        <oboInOwl:id>GAZ:00193785</oboInOwl:id>
        <rdfs:label>Banias River</rdfs:label>
    </owl:NamedIndividual>
    


    <!-- http://purl.obolibrary.org/obo/GAZ_00193791 -->

    <owl:NamedIndividual rdf:about="http://purl.obolibrary.org/obo/GAZ_00193791">
        <obo:IAO_0000115>The lowest nature reserve in the world, with a spectacular array of scenery near the east cost of the Dead Sea. The reserve is located within the deep Wadi Mujib gorge, which enters the Dead Sea at 410 m below sea level. The Reserve extends to the Kerak and Madaba mountains to the north and south.</obo:IAO_0000115>
        <oboInOwl:hasOBONamespace>GAZ</oboInOwl:hasOBONamespace>
        <oboInOwl:id>GAZ:00193791</oboInOwl:id>
        <rdfs:label>Mujib Nature Reserve</rdfs:label>
    </owl:NamedIndividual>
    


    <!-- http://purl.obolibrary.org/obo/GAZ_00193804 -->

    <owl:NamedIndividual rdf:about="http://purl.obolibrary.org/obo/GAZ_00193804">
        <obo:RO_0001025 rdf:resource="http://purl.obolibrary.org/obo/GAZ_00007862"/>
        <obo:IAO_0000115>A protected area located on the Red Sea south of Eilat.</obo:IAO_0000115>
        <oboInOwl:hasOBONamespace>GAZ</oboInOwl:hasOBONamespace>
        <oboInOwl:id>GAZ:00193804</oboInOwl:id>
        <rdfs:label>Coral Beach Nature Reserve</rdfs:label>
    </owl:NamedIndividual>
    


    <!-- http://purl.obolibrary.org/obo/GAZ_00193854 -->

    <owl:NamedIndividual rdf:about="http://purl.obolibrary.org/obo/GAZ_00193854">
        <obo:RO_0001025 rdf:resource="http://purl.obolibrary.org/obo/GAZ_00010533"/>
        <obo:IAO_0000115>A protected area. An archeological site. A World Heritage Site.</obo:IAO_0000115>
        <oboInOwl:hasOBONamespace>GAZ</oboInOwl:hasOBONamespace>
        <oboInOwl:id>GAZ:00193854</oboInOwl:id>
        <rdfs:label>Megiddo National Park</rdfs:label>
    </owl:NamedIndividual>
    


    <!-- http://purl.obolibrary.org/obo/GAZ_00193855 -->

    <owl:NamedIndividual rdf:about="http://purl.obolibrary.org/obo/GAZ_00193855">
        <obo:RO_0001025 rdf:resource="http://purl.obolibrary.org/obo/GAZ_00010533"/>
        <obo:IAO_0000115>A protected area. An archeological site.</obo:IAO_0000115>
        <oboInOwl:hasOBONamespace>GAZ</oboInOwl:hasOBONamespace>
        <oboInOwl:id>GAZ:00193855</oboInOwl:id>
        <rdfs:label>Ma&apos;ayan Harod National Park</rdfs:label>
    </owl:NamedIndividual>
    


    <!-- http://purl.obolibrary.org/obo/GAZ_00193856 -->

    <owl:NamedIndividual rdf:about="http://purl.obolibrary.org/obo/GAZ_00193856">
        <obo:RO_0001025 rdf:resource="http://purl.obolibrary.org/obo/GAZ_00193855"/>
        <obo:IAO_0000115>A spring. It emerges from a rocky cave on the slope of Mount Gilboa.</obo:IAO_0000115>
        <oboInOwl:hasOBONamespace>GAZ</oboInOwl:hasOBONamespace>
        <oboInOwl:id>GAZ:00193856</oboInOwl:id>
        <rdfs:label>Ma&apos;ayan Harod</rdfs:label>
    </owl:NamedIndividual>
    


    <!-- http://purl.obolibrary.org/obo/GAZ_00193866 -->

    <owl:NamedIndividual rdf:about="http://purl.obolibrary.org/obo/GAZ_00193866">
        <obo:RO_0001025 rdf:resource="http://purl.obolibrary.org/obo/GAZ_00044915"/>
        <obo:IAO_0000115>A protected area. An archeological site.</obo:IAO_0000115>
        <oboInOwl:hasOBONamespace>GAZ</oboInOwl:hasOBONamespace>
        <oboInOwl:id>GAZ:00193866</oboInOwl:id>
        <rdfs:label>Bet She&apos;an National Park</rdfs:label>
    </owl:NamedIndividual>
    


    <!-- http://purl.obolibrary.org/obo/GAZ_00193885 -->

    <owl:NamedIndividual rdf:about="http://purl.obolibrary.org/obo/GAZ_00193885">
        <obo:RO_0001025 rdf:resource="http://purl.obolibrary.org/obo/GAZ_00008742"/>
        <obo:IAO_0000115>A protected area.</obo:IAO_0000115>
        <oboInOwl:hasOBONamespace>GAZ</oboInOwl:hasOBONamespace>
        <oboInOwl:id>GAZ:00193885</oboInOwl:id>
        <rdfs:label>Hurshat Tal National Park</rdfs:label>
    </owl:NamedIndividual>
    


    <!-- http://purl.obolibrary.org/obo/GAZ_00193886 -->

    <owl:NamedIndividual rdf:about="http://purl.obolibrary.org/obo/GAZ_00193886">
        <obo:RO_0001025 rdf:resource="http://purl.obolibrary.org/obo/GAZ_00008742"/>
        <obo:IAO_0000115>A protected area.</obo:IAO_0000115>
        <oboInOwl:hasOBONamespace>GAZ</oboInOwl:hasOBONamespace>
        <oboInOwl:id>GAZ:00193886</oboInOwl:id>
        <rdfs:label>Hula Nature Reserve</rdfs:label>
    </owl:NamedIndividual>
    


    <!-- http://purl.obolibrary.org/obo/GAZ_00193951 -->

    <owl:NamedIndividual rdf:about="http://purl.obolibrary.org/obo/GAZ_00193951">
        <obo:RO_0001025 rdf:resource="http://purl.obolibrary.org/obo/GAZ_00044915"/>
        <obo:IAO_0000115>A large spit of land which now separates the North and the South basins of the Dead Sea. Entirely located in Jordan.</obo:IAO_0000115>
        <oboInOwl:hasOBONamespace>GAZ</oboInOwl:hasOBONamespace>
        <oboInOwl:id>GAZ:00193951</oboInOwl:id>
        <rdfs:label>Lisan Peninsula</rdfs:label>
    </owl:NamedIndividual>
    


    <!-- http://purl.obolibrary.org/obo/GAZ_00230341 -->

    <owl:NamedIndividual rdf:about="http://purl.obolibrary.org/obo/GAZ_00230341">
        <obo:RO_0001025 rdf:resource="http://purl.obolibrary.org/obo/GAZ_00051205"/>
        <obo:IAO_0000115>A lake. Located in the Northern Red Sea Region, Lake Kulul lies in the Eritrean portion of the Afar Depression.</obo:IAO_0000115>
        <oboInOwl:hasOBONamespace>GAZ</oboInOwl:hasOBONamespace>
        <oboInOwl:id>GAZ:00230341</oboInOwl:id>
        <rdfs:label>Lake Kulul</rdfs:label>
    </owl:NamedIndividual>
    


    <!-- http://purl.obolibrary.org/obo/GAZ_00230365 -->

    <owl:NamedIndividual rdf:about="http://purl.obolibrary.org/obo/GAZ_00230365">
        <obo:IAO_0000115>A river of southern Ethiopia. Located inside Omo National Park, it is a tributary of the Omo River.</obo:IAO_0000115>
        <oboInOwl:hasOBONamespace>GAZ</oboInOwl:hasOBONamespace>
        <oboInOwl:id>GAZ:00230365</oboInOwl:id>
        <rdfs:label>Mui River</rdfs:label>
    </owl:NamedIndividual>
    


    <!-- http://purl.obolibrary.org/obo/GAZ_00230369 -->

    <owl:NamedIndividual rdf:about="http://purl.obolibrary.org/obo/GAZ_00230369">
        <obo:IAO_0000115>A river of southern Ethiopia, entirely located in the Debub Omo Zone of the Southern Nations, Nationalities, and People&apos;s Region. It is a tributary of the Omo River.</obo:IAO_0000115>
        <oboInOwl:hasOBONamespace>GAZ</oboInOwl:hasOBONamespace>
        <oboInOwl:id>GAZ:00230369</oboInOwl:id>
        <rdfs:label>Mago River</rdfs:label>
    </owl:NamedIndividual>
    


    <!-- http://purl.obolibrary.org/obo/GAZ_00230372 -->

    <owl:NamedIndividual rdf:about="http://purl.obolibrary.org/obo/GAZ_00230372">
        <obo:IAO_0000115>A hydroelectric dam. Completed 2004.</obo:IAO_0000115>
        <oboInOwl:hasOBONamespace>GAZ</oboInOwl:hasOBONamespace>
        <oboInOwl:id>GAZ:00230372</oboInOwl:id>
        <rdfs:label>Gojeb Dam</rdfs:label>
    </owl:NamedIndividual>
    


    <!-- http://purl.obolibrary.org/obo/GAZ_00230373 -->

    <owl:NamedIndividual rdf:about="http://purl.obolibrary.org/obo/GAZ_00230373">
        <obo:RO_0001025 rdf:resource="http://purl.obolibrary.org/obo/GAZ_00052567"/>
        <obo:IAO_0000115>A river. A tributary of the Omo River.</obo:IAO_0000115>
        <oboInOwl:hasOBONamespace>GAZ</oboInOwl:hasOBONamespace>
        <oboInOwl:id>GAZ:00230373</oboInOwl:id>
        <rdfs:label>Wabi River</rdfs:label>
    </owl:NamedIndividual>
    


    <!-- http://purl.obolibrary.org/obo/GAZ_00230374 -->

    <owl:NamedIndividual rdf:about="http://purl.obolibrary.org/obo/GAZ_00230374">
        <obo:RO_0001025 rdf:resource="http://purl.obolibrary.org/obo/GAZ_00052567"/>
        <obo:IAO_0000115>A hydroelectric dam.</obo:IAO_0000115>
        <oboInOwl:hasOBONamespace>GAZ</oboInOwl:hasOBONamespace>
        <oboInOwl:id>GAZ:00230374</oboInOwl:id>
        <rdfs:label>Gibe III Dam</rdfs:label>
    </owl:NamedIndividual>
    


    <!-- http://purl.obolibrary.org/obo/GAZ_00230375 -->

    <owl:NamedIndividual rdf:about="http://purl.obolibrary.org/obo/GAZ_00230375">
        <obo:IAO_0000115>A hydroelectric dam. Constructed 1986-2004.</obo:IAO_0000115>
        <oboInOwl:hasOBONamespace>GAZ</oboInOwl:hasOBONamespace>
        <oboInOwl:id>GAZ:00230375</oboInOwl:id>
        <rdfs:label>Gilgel Gibe Dam</rdfs:label>
    </owl:NamedIndividual>
    


    <!-- http://purl.obolibrary.org/obo/GAZ_00230429 -->

    <owl:NamedIndividual rdf:about="http://purl.obolibrary.org/obo/GAZ_00230429">
        <obo:IAO_0000115>A river of south-central Ethiopia. It rises on the southwestern slopes of Mount Gurage, flowing south along the western side of the Great Rift Valley, to empty into Lake Abaya.</obo:IAO_0000115>
        <oboInOwl:hasOBONamespace>GAZ</oboInOwl:hasOBONamespace>
        <oboInOwl:id>GAZ:00230429</oboInOwl:id>
        <rdfs:label>Bilate River</rdfs:label>
    </owl:NamedIndividual>
    


    <!-- http://purl.obolibrary.org/obo/GAZ_00230463 -->

    <owl:NamedIndividual rdf:about="http://purl.obolibrary.org/obo/GAZ_00230463">
        <obo:IAO_0000115>A river in central Ethiopia. It empties into Lake Zway.</obo:IAO_0000115>
        <oboInOwl:hasOBONamespace>GAZ</oboInOwl:hasOBONamespace>
        <oboInOwl:id>GAZ:00230463</oboInOwl:id>
        <rdfs:label>Meki River</rdfs:label>
    </owl:NamedIndividual>
    


    <!-- http://purl.obolibrary.org/obo/GAZ_00233544 -->

    <owl:NamedIndividual rdf:about="http://purl.obolibrary.org/obo/GAZ_00233544">
        <obo:RO_0001025 rdf:resource="http://purl.obolibrary.org/obo/GAZ_00005375"/>
        <obo:IAO_0000115>A region in northeastern Uganda comprising the five districts of Abim, Kaabong, Kotido, Moroto and Nakapiripirit. Kaabong is on the northeastern borders to Sudan and Kenya, and is home to the Kidepo Valley National Park, Nakapiripirit is the most-eastern one, bordering Mount Elgon National Park.</obo:IAO_0000115>
        <oboInOwl:hasOBONamespace>GAZ</oboInOwl:hasOBONamespace>
        <oboInOwl:id>GAZ:00233544</oboInOwl:id>
        <rdfs:label>Karamoja Subregion</rdfs:label>
    </owl:NamedIndividual>
    


    <!-- http://purl.obolibrary.org/obo/GAZ_00233545 -->

    <owl:NamedIndividual rdf:about="http://purl.obolibrary.org/obo/GAZ_00233545">
        <obo:RO_0001025 rdf:resource="http://purl.obolibrary.org/obo/GAZ_00015504"/>
        <oboInOwl:hasOBONamespace>GAZ</oboInOwl:hasOBONamespace>
        <oboInOwl:id>GAZ:00233545</oboInOwl:id>
        <rdfs:label>Bokora County</rdfs:label>
    </owl:NamedIndividual>
    


    <!-- http://purl.obolibrary.org/obo/GAZ_00233546 -->

    <owl:NamedIndividual rdf:about="http://purl.obolibrary.org/obo/GAZ_00233546">
        <obo:RO_0001025 rdf:resource="http://purl.obolibrary.org/obo/GAZ_00015504"/>
        <oboInOwl:hasOBONamespace>GAZ</oboInOwl:hasOBONamespace>
        <oboInOwl:id>GAZ:00233546</oboInOwl:id>
        <rdfs:label>Matheniko County</rdfs:label>
    </owl:NamedIndividual>
    


    <!-- http://purl.obolibrary.org/obo/GAZ_00233547 -->

    <owl:NamedIndividual rdf:about="http://purl.obolibrary.org/obo/GAZ_00233547">
        <obo:RO_0001025 rdf:resource="http://purl.obolibrary.org/obo/GAZ_00015504"/>
        <oboInOwl:hasOBONamespace>GAZ</oboInOwl:hasOBONamespace>
        <oboInOwl:id>GAZ:00233547</oboInOwl:id>
        <rdfs:label>Municipality of Moroto</rdfs:label>
    </owl:NamedIndividual>
    


    <!-- http://purl.obolibrary.org/obo/GAZ_00234085 -->

    <owl:NamedIndividual rdf:about="http://purl.obolibrary.org/obo/GAZ_00234085">
        <obo:IAO_0000115>A hydroelectric dam. Located at the Ruzizi River outlet from Lake Kivu. Constructed 1958.</obo:IAO_0000115>
        <oboInOwl:hasOBONamespace>GAZ</oboInOwl:hasOBONamespace>
        <oboInOwl:id>GAZ:00234085</oboInOwl:id>
        <rdfs:label>Ruzizi I Hydroelectric Dam</rdfs:label>
    </owl:NamedIndividual>
    


    <!-- http://purl.obolibrary.org/obo/GAZ_00234089 -->

    <owl:NamedIndividual rdf:about="http://purl.obolibrary.org/obo/GAZ_00234089">
        <obo:IAO_0000115>Water falls.</obo:IAO_0000115>
        <oboInOwl:hasOBONamespace>GAZ</oboInOwl:hasOBONamespace>
        <oboInOwl:id>GAZ:00234089</oboInOwl:id>
        <rdfs:label>Chutes de la Kagera</rdfs:label>
    </owl:NamedIndividual>
    


    <!-- http://purl.obolibrary.org/obo/GAZ_00235791 -->

    <owl:NamedIndividual rdf:about="http://purl.obolibrary.org/obo/GAZ_00235791">
        <obo:IAO_0000115>A river. A tributary of the Kagera River.</obo:IAO_0000115>
        <oboInOwl:hasOBONamespace>GAZ</oboInOwl:hasOBONamespace>
        <oboInOwl:id>GAZ:00235791</oboInOwl:id>
        <rdfs:label>Muvumba River</rdfs:label>
    </owl:NamedIndividual>
    


    <!-- http://purl.obolibrary.org/obo/GAZ_00235792 -->

    <owl:NamedIndividual rdf:about="http://purl.obolibrary.org/obo/GAZ_00235792">
        <oboInOwl:hasOBONamespace>GAZ</oboInOwl:hasOBONamespace>
        <oboInOwl:id>GAZ:00235792</oboInOwl:id>
        <rdfs:label>Karangaza River</rdfs:label>
    </owl:NamedIndividual>
    


    <!-- http://purl.obolibrary.org/obo/GAZ_00235793 -->

    <owl:NamedIndividual rdf:about="http://purl.obolibrary.org/obo/GAZ_00235793">
        <oboInOwl:hasOBONamespace>GAZ</oboInOwl:hasOBONamespace>
        <oboInOwl:id>GAZ:00235793</oboInOwl:id>
        <rdfs:label>Kamiramugezi River</rdfs:label>
    </owl:NamedIndividual>
    


    <!-- http://purl.obolibrary.org/obo/GAZ_00235795 -->

    <owl:NamedIndividual rdf:about="http://purl.obolibrary.org/obo/GAZ_00235795">
        <obo:IAO_0000115>A river flowing into Lake Kivu.</obo:IAO_0000115>
        <oboInOwl:hasOBONamespace>GAZ</oboInOwl:hasOBONamespace>
        <oboInOwl:id>GAZ:00235795</oboInOwl:id>
        <rdfs:label>Kalundura River</rdfs:label>
    </owl:NamedIndividual>
    


    <!-- http://purl.obolibrary.org/obo/GAZ_00236097 -->

    <owl:NamedIndividual rdf:about="http://purl.obolibrary.org/obo/GAZ_00236097">
        <obo:RO_0001025 rdf:resource="http://purl.obolibrary.org/obo/GAZ_00000007"/>
        <obo:IAO_0000115>An arid part of the Great Rift Valley in Kenya, directly south of Lake Turkana. The valley is floored by a seasonal stream complex, the Suguta River, that terminates in the seasonal playa Lake Alablab. Lake Logipi, a saline, alkaline lake lies at the northern end of the valley, where it is separated from Lake Turkana by a complex series of volcanoes called the Barrier.</obo:IAO_0000115>
        <oboInOwl:hasOBONamespace>GAZ</oboInOwl:hasOBONamespace>
        <oboInOwl:id>GAZ:00236097</oboInOwl:id>
        <rdfs:label>Suguta Valley</rdfs:label>
    </owl:NamedIndividual>
    


    <!-- http://purl.obolibrary.org/obo/GAZ_00236098 -->

    <owl:NamedIndividual rdf:about="http://purl.obolibrary.org/obo/GAZ_00236098">
        <obo:RO_0001025 rdf:resource="http://purl.obolibrary.org/obo/GAZ_00236097"/>
        <obo:IAO_0000115>A seasonal playa lake.</obo:IAO_0000115>
        <oboInOwl:hasOBONamespace>GAZ</oboInOwl:hasOBONamespace>
        <oboInOwl:id>GAZ:00236098</oboInOwl:id>
        <rdfs:label>Lake Alablab</rdfs:label>
    </owl:NamedIndividual>
    


    <!-- http://purl.obolibrary.org/obo/GAZ_00236099 -->

    <owl:NamedIndividual rdf:about="http://purl.obolibrary.org/obo/GAZ_00236099">
        <obo:RO_0001025 rdf:resource="http://purl.obolibrary.org/obo/GAZ_00236097"/>
        <obo:IAO_0000115>An intermittent river.</obo:IAO_0000115>
        <oboInOwl:hasOBONamespace>GAZ</oboInOwl:hasOBONamespace>
        <oboInOwl:id>GAZ:00236099</oboInOwl:id>
        <rdfs:label>Suguta River</rdfs:label>
    </owl:NamedIndividual>
    


    <!-- http://purl.obolibrary.org/obo/GAZ_00236105 -->

    <owl:NamedIndividual rdf:about="http://purl.obolibrary.org/obo/GAZ_00236105">
        <obo:RO_0001025 rdf:resource="http://purl.obolibrary.org/obo/GAZ_00000007"/>
        <obo:IAO_0000115>A fault-scarp caused by to post-Miocene faulting and there are Miocene beds visible. The escarpment is part of the western wall of the Great Rift Valley.</obo:IAO_0000115>
        <oboInOwl:hasOBONamespace>GAZ</oboInOwl:hasOBONamespace>
        <oboInOwl:id>GAZ:00236105</oboInOwl:id>
        <rdfs:label>Elgeyo Escarpment</rdfs:label>
    </owl:NamedIndividual>
    


    <!-- http://purl.obolibrary.org/obo/GAZ_00236116 -->

    <owl:NamedIndividual rdf:about="http://purl.obolibrary.org/obo/GAZ_00236116">
        <obo:RO_0001025 rdf:resource="http://purl.obolibrary.org/obo/GAZ_00000007"/>
        <obo:IAO_0000115>Peaks in a ridge along the Great Rift Valley, located southwest near Nairobi, in southern Kenya.</obo:IAO_0000115>
        <oboInOwl:hasOBONamespace>GAZ</oboInOwl:hasOBONamespace>
        <oboInOwl:id>GAZ:00236116</oboInOwl:id>
        <rdfs:label>Ngong Hills</rdfs:label>
    </owl:NamedIndividual>
    


    <!-- http://purl.obolibrary.org/obo/GAZ_00236121 -->

    <owl:NamedIndividual rdf:about="http://purl.obolibrary.org/obo/GAZ_00236121">
        <rdf:type rdf:resource="http://purl.obolibrary.org/obo/ENVO_00000100"/>
        <rdf:type rdf:resource="http://purl.obolibrary.org/obo/ENVO_00000479"/>
        <obo:RO_0001025 rdf:resource="http://purl.obolibrary.org/obo/GAZ_00076405"/>
        <obo:IAO_0000115>A gorge. A former outlet of Lake Naivasha.</obo:IAO_0000115>
        <oboInOwl:hasOBONamespace>GAZ</oboInOwl:hasOBONamespace>
        <oboInOwl:id>GAZ:00236121</oboInOwl:id>
        <rdfs:label>Njorowa Gorge</rdfs:label>
    </owl:NamedIndividual>
    


    <!-- http://purl.obolibrary.org/obo/GAZ_00236122 -->

    <owl:NamedIndividual rdf:about="http://purl.obolibrary.org/obo/GAZ_00236122">
        <obo:RO_0001025 rdf:resource="http://purl.obolibrary.org/obo/GAZ_00000007"/>
        <obo:IAO_0000115>A highland area of lush green rolling hills at the edge of the Great Rift Valley in the Rift Valley Province of Kenya.</obo:IAO_0000115>
        <oboInOwl:hasOBONamespace>GAZ</oboInOwl:hasOBONamespace>
        <oboInOwl:id>GAZ:00236122</oboInOwl:id>
        <rdfs:label>Nandi Hills</rdfs:label>
    </owl:NamedIndividual>
    


    <!-- http://purl.obolibrary.org/obo/GAZ_00236131 -->

    <owl:NamedIndividual rdf:about="http://purl.obolibrary.org/obo/GAZ_00236131">
        <obo:IAO_0000115>A peak of Mount Elgon.</obo:IAO_0000115>
        <oboInOwl:hasOBONamespace>GAZ</oboInOwl:hasOBONamespace>
        <oboInOwl:id>GAZ:00236131</oboInOwl:id>
        <rdfs:label>Wagagai</rdfs:label>
    </owl:NamedIndividual>
    


    <!-- http://purl.obolibrary.org/obo/GAZ_00236132 -->

    <owl:NamedIndividual rdf:about="http://purl.obolibrary.org/obo/GAZ_00236132">
        <obo:IAO_0000115>A peak of Mount Elgon.</obo:IAO_0000115>
        <oboInOwl:hasOBONamespace>GAZ</oboInOwl:hasOBONamespace>
        <oboInOwl:id>GAZ:00236132</oboInOwl:id>
        <rdfs:label>Sudek</rdfs:label>
    </owl:NamedIndividual>
    


    <!-- http://purl.obolibrary.org/obo/GAZ_00236133 -->

    <owl:NamedIndividual rdf:about="http://purl.obolibrary.org/obo/GAZ_00236133">
        <obo:IAO_0000115>A peak of Mount Elgon.</obo:IAO_0000115>
        <oboInOwl:hasOBONamespace>GAZ</oboInOwl:hasOBONamespace>
        <oboInOwl:id>GAZ:00236133</oboInOwl:id>
        <rdfs:label>Koitobos</rdfs:label>
    </owl:NamedIndividual>
    


    <!-- http://purl.obolibrary.org/obo/GAZ_00236134 -->

    <owl:NamedIndividual rdf:about="http://purl.obolibrary.org/obo/GAZ_00236134">
        <obo:IAO_0000115>A peak of Mount Elgon.</obo:IAO_0000115>
        <oboInOwl:hasOBONamespace>GAZ</oboInOwl:hasOBONamespace>
        <oboInOwl:id>GAZ:00236134</oboInOwl:id>
        <rdfs:label>Mubiyi</rdfs:label>
    </owl:NamedIndividual>
    


    <!-- http://purl.obolibrary.org/obo/GAZ_00236135 -->

    <owl:NamedIndividual rdf:about="http://purl.obolibrary.org/obo/GAZ_00236135">
        <obo:IAO_0000115>A peak of Mount Elgon.</obo:IAO_0000115>
        <oboInOwl:hasOBONamespace>GAZ</oboInOwl:hasOBONamespace>
        <oboInOwl:id>GAZ:00236135</oboInOwl:id>
        <rdfs:label>Masaba</rdfs:label>
    </owl:NamedIndividual>
    


    <!-- http://purl.obolibrary.org/obo/GAZ_00236136 -->

    <owl:NamedIndividual rdf:about="http://purl.obolibrary.org/obo/GAZ_00236136">
        <obo:RO_0001025 rdf:resource="http://purl.obolibrary.org/obo/GAZ_00076409"/>
        <obo:IAO_0000115>A non-solutional cave.</obo:IAO_0000115>
        <oboInOwl:hasOBONamespace>GAZ</oboInOwl:hasOBONamespace>
        <oboInOwl:id>GAZ:00236136</oboInOwl:id>
        <rdfs:label>Ngwarisha Cave</rdfs:label>
    </owl:NamedIndividual>
    


    <!-- http://purl.obolibrary.org/obo/GAZ_00236137 -->

    <owl:NamedIndividual rdf:about="http://purl.obolibrary.org/obo/GAZ_00236137">
        <obo:RO_0001025 rdf:resource="http://purl.obolibrary.org/obo/GAZ_00076409"/>
        <obo:IAO_0000115>A non-solutional cave.</obo:IAO_0000115>
        <oboInOwl:hasOBONamespace>GAZ</oboInOwl:hasOBONamespace>
        <oboInOwl:id>GAZ:00236137</oboInOwl:id>
        <rdfs:label>Makingeny Cave</rdfs:label>
    </owl:NamedIndividual>
    


    <!-- http://purl.obolibrary.org/obo/GAZ_00236138 -->

    <owl:NamedIndividual rdf:about="http://purl.obolibrary.org/obo/GAZ_00236138">
        <obo:RO_0001025 rdf:resource="http://purl.obolibrary.org/obo/GAZ_00076409"/>
        <obo:IAO_0000115>A non-solutional cave.</obo:IAO_0000115>
        <oboInOwl:hasOBONamespace>GAZ</oboInOwl:hasOBONamespace>
        <oboInOwl:id>GAZ:00236138</oboInOwl:id>
        <rdfs:label>Chepnyalil Cave</rdfs:label>
    </owl:NamedIndividual>
    


    <!-- http://purl.obolibrary.org/obo/GAZ_00236139 -->

    <owl:NamedIndividual rdf:about="http://purl.obolibrary.org/obo/GAZ_00236139">
        <obo:RO_0001025 rdf:resource="http://purl.obolibrary.org/obo/GAZ_00076409"/>
        <obo:IAO_0000115>A non-solutional cave.</obo:IAO_0000115>
        <oboInOwl:hasOBONamespace>GAZ</oboInOwl:hasOBONamespace>
        <oboInOwl:id>GAZ:00236139</oboInOwl:id>
        <rdfs:label>Kiptoro Cave</rdfs:label>
    </owl:NamedIndividual>
    


    <!-- http://purl.obolibrary.org/obo/GAZ_00236170 -->

    <owl:NamedIndividual rdf:about="http://purl.obolibrary.org/obo/GAZ_00236170">
        <obo:RO_0001025 rdf:resource="http://purl.obolibrary.org/obo/GAZ_00052895"/>
        <obo:IAO_0000115>A bay.</obo:IAO_0000115>
        <oboInOwl:hasOBONamespace>GAZ</oboInOwl:hasOBONamespace>
        <oboInOwl:id>GAZ:00236170</oboInOwl:id>
        <rdfs:label>Naya Bay</rdfs:label>
    </owl:NamedIndividual>
    


    <!-- http://purl.obolibrary.org/obo/GAZ_00236171 -->

    <owl:NamedIndividual rdf:about="http://purl.obolibrary.org/obo/GAZ_00236171">
        <obo:RO_0001025 rdf:resource="http://purl.obolibrary.org/obo/GAZ_00052895"/>
        <obo:IAO_0000115>A bay.</obo:IAO_0000115>
        <oboInOwl:hasOBONamespace>GAZ</oboInOwl:hasOBONamespace>
        <oboInOwl:id>GAZ:00236171</oboInOwl:id>
        <rdfs:label>Nyakach Bay</rdfs:label>
    </owl:NamedIndividual>
    


    <!-- http://purl.obolibrary.org/obo/GAZ_00236172 -->

    <owl:NamedIndividual rdf:about="http://purl.obolibrary.org/obo/GAZ_00236172">
        <obo:RO_0001025 rdf:resource="http://purl.obolibrary.org/obo/GAZ_00052895"/>
        <obo:IAO_0000115>A bay.</obo:IAO_0000115>
        <oboInOwl:hasOBONamespace>GAZ</oboInOwl:hasOBONamespace>
        <oboInOwl:id>GAZ:00236172</oboInOwl:id>
        <rdfs:label>Osodo Bay</rdfs:label>
    </owl:NamedIndividual>
    


    <!-- http://purl.obolibrary.org/obo/GAZ_00236173 -->

    <owl:NamedIndividual rdf:about="http://purl.obolibrary.org/obo/GAZ_00236173">
        <obo:RO_0001025 rdf:resource="http://purl.obolibrary.org/obo/GAZ_00052895"/>
        <obo:IAO_0000115>A bay.</obo:IAO_0000115>
        <oboInOwl:hasOBONamespace>GAZ</oboInOwl:hasOBONamespace>
        <oboInOwl:id>GAZ:00236173</oboInOwl:id>
        <rdfs:label>Kendu Bay</rdfs:label>
    </owl:NamedIndividual>
    


    <!-- http://purl.obolibrary.org/obo/GAZ_00236174 -->

    <owl:NamedIndividual rdf:about="http://purl.obolibrary.org/obo/GAZ_00236174">
        <obo:RO_0001025 rdf:resource="http://purl.obolibrary.org/obo/GAZ_00052895"/>
        <obo:IAO_0000115>A bay.</obo:IAO_0000115>
        <oboInOwl:hasOBONamespace>GAZ</oboInOwl:hasOBONamespace>
        <oboInOwl:id>GAZ:00236174</oboInOwl:id>
        <rdfs:label>Ruri Bay</rdfs:label>
    </owl:NamedIndividual>
    


    <!-- http://purl.obolibrary.org/obo/GAZ_00236175 -->

    <owl:NamedIndividual rdf:about="http://purl.obolibrary.org/obo/GAZ_00236175">
        <obo:RO_0001025 rdf:resource="http://purl.obolibrary.org/obo/GAZ_00052895"/>
        <obo:IAO_0000115>A bay.</obo:IAO_0000115>
        <oboInOwl:hasOBONamespace>GAZ</oboInOwl:hasOBONamespace>
        <oboInOwl:id>GAZ:00236175</oboInOwl:id>
        <rdfs:label>Mirunda Bay</rdfs:label>
    </owl:NamedIndividual>
    


    <!-- http://purl.obolibrary.org/obo/GAZ_00236176 -->

    <owl:NamedIndividual rdf:about="http://purl.obolibrary.org/obo/GAZ_00236176">
        <obo:RO_0001025 rdf:resource="http://purl.obolibrary.org/obo/GAZ_00052895"/>
        <obo:IAO_0000115>A bay.</obo:IAO_0000115>
        <oboInOwl:hasOBONamespace>GAZ</oboInOwl:hasOBONamespace>
        <oboInOwl:id>GAZ:00236176</oboInOwl:id>
        <rdfs:label>Olambwe Bay</rdfs:label>
    </owl:NamedIndividual>
    


    <!-- http://purl.obolibrary.org/obo/GAZ_00236183 -->

    <owl:NamedIndividual rdf:about="http://purl.obolibrary.org/obo/GAZ_00236183">
        <obo:RO_0001025 rdf:resource="http://purl.obolibrary.org/obo/GAZ_00008411"/>
        <obo:IAO_0000115>An alkaline hot spring running into Lake Bogoria.</obo:IAO_0000115>
        <oboInOwl:hasOBONamespace>GAZ</oboInOwl:hasOBONamespace>
        <oboInOwl:id>GAZ:00236183</oboInOwl:id>
        <rdfs:label>Loburu</rdfs:label>
    </owl:NamedIndividual>
    


    <!-- http://purl.obolibrary.org/obo/GAZ_00236184 -->

    <owl:NamedIndividual rdf:about="http://purl.obolibrary.org/obo/GAZ_00236184">
        <obo:RO_0001025 rdf:resource="http://purl.obolibrary.org/obo/GAZ_00008411"/>
        <obo:IAO_0000115>An alkaline hot spring running into Lake Bogoria.</obo:IAO_0000115>
        <oboInOwl:hasOBONamespace>GAZ</oboInOwl:hasOBONamespace>
        <oboInOwl:id>GAZ:00236184</oboInOwl:id>
        <rdfs:label>Chemurkeu</rdfs:label>
    </owl:NamedIndividual>
    


    <!-- http://purl.obolibrary.org/obo/GAZ_00236185 -->

    <owl:NamedIndividual rdf:about="http://purl.obolibrary.org/obo/GAZ_00236185">
        <obo:RO_0001025 rdf:resource="http://purl.obolibrary.org/obo/GAZ_00008411"/>
        <obo:IAO_0000115>A group of alkaline hot spring running into Lake Bogoria.</obo:IAO_0000115>
        <oboInOwl:hasOBONamespace>GAZ</oboInOwl:hasOBONamespace>
        <oboInOwl:id>GAZ:00236185</oboInOwl:id>
        <rdfs:label>Southern group of hot springs</rdfs:label>
    </owl:NamedIndividual>
    


    <!-- http://purl.obolibrary.org/obo/GAZ_00236186 -->

    <owl:NamedIndividual rdf:about="http://purl.obolibrary.org/obo/GAZ_00236186">
        <obo:RO_0001025 rdf:resource="http://purl.obolibrary.org/obo/GAZ_00236185"/>
        <obo:IAO_0000115>An alkaline hot spring running into Lake Bogoria.</obo:IAO_0000115>
        <oboInOwl:hasOBONamespace>GAZ</oboInOwl:hasOBONamespace>
        <oboInOwl:id>GAZ:00236186</oboInOwl:id>
        <rdfs:label>Ng&apos;wasis</rdfs:label>
    </owl:NamedIndividual>
    


    <!-- http://purl.obolibrary.org/obo/GAZ_00236187 -->

    <owl:NamedIndividual rdf:about="http://purl.obolibrary.org/obo/GAZ_00236187">
        <obo:RO_0001025 rdf:resource="http://purl.obolibrary.org/obo/GAZ_00236185"/>
        <obo:IAO_0000115>An alkaline hot spring running into Lake Bogoria.</obo:IAO_0000115>
        <oboInOwl:hasOBONamespace>GAZ</oboInOwl:hasOBONamespace>
        <oboInOwl:id>GAZ:00236187</oboInOwl:id>
        <rdfs:label>Koibobei</rdfs:label>
    </owl:NamedIndividual>
    


    <!-- http://purl.obolibrary.org/obo/GAZ_00236188 -->

    <owl:NamedIndividual rdf:about="http://purl.obolibrary.org/obo/GAZ_00236188">
        <obo:RO_0001025 rdf:resource="http://purl.obolibrary.org/obo/GAZ_00236185"/>
        <obo:IAO_0000115>An alkaline hot spring running into Lake Bogoria.</obo:IAO_0000115>
        <oboInOwl:hasOBONamespace>GAZ</oboInOwl:hasOBONamespace>
        <oboInOwl:id>GAZ:00236188</oboInOwl:id>
        <rdfs:label>Losaramat</rdfs:label>
    </owl:NamedIndividual>
    


    <!-- http://purl.obolibrary.org/obo/GAZ_00236192 -->

    <owl:NamedIndividual rdf:about="http://purl.obolibrary.org/obo/GAZ_00236192">
        <obo:RO_0001025 rdf:resource="http://purl.obolibrary.org/obo/GAZ_00000007"/>
        <obo:IAO_0000115>An escarpment in southern Kenya. The escarpment is around 50 km long and elongated in N-W direction. Its northern edge approximately 120 km southwest of Nairobi, while the southern edge is near the Tanzanian border, at the northwestern corner of Lake Natron. The southern Ewaso Ngiro river flows along the foot of the escarpment, while Loita Hills are located west of the escarpment . The escarpment forms the western wall of the Great Rift Valley.</obo:IAO_0000115>
        <oboInOwl:hasOBONamespace>GAZ</oboInOwl:hasOBONamespace>
        <oboInOwl:id>GAZ:00236192</oboInOwl:id>
        <rdfs:label>Nguruman Escarpment</rdfs:label>
    </owl:NamedIndividual>
    


    <!-- http://purl.obolibrary.org/obo/GAZ_00236193 -->

    <owl:NamedIndividual rdf:about="http://purl.obolibrary.org/obo/GAZ_00236193">
        <obo:RO_0001025 rdf:resource="http://purl.obolibrary.org/obo/GAZ_00236192"/>
        <obo:IAO_0000115>A protected area.</obo:IAO_0000115>
        <oboInOwl:hasOBONamespace>GAZ</oboInOwl:hasOBONamespace>
        <oboInOwl:id>GAZ:00236193</oboInOwl:id>
        <rdfs:label>Shompole Conservancy</rdfs:label>
    </owl:NamedIndividual>
    


    <!-- http://purl.obolibrary.org/obo/GAZ_00236194 -->

    <owl:NamedIndividual rdf:about="http://purl.obolibrary.org/obo/GAZ_00236194">
        <obo:IAO_0000115>A river in Rift Valley Province, Kenya. It flows northward into Lake Turkana.</obo:IAO_0000115>
        <oboInOwl:hasOBONamespace>GAZ</oboInOwl:hasOBONamespace>
        <oboInOwl:id>GAZ:00236194</oboInOwl:id>
        <rdfs:label>Kerio River</rdfs:label>
    </owl:NamedIndividual>
    


    <!-- http://purl.obolibrary.org/obo/GAZ_00236202 -->

    <owl:NamedIndividual rdf:about="http://purl.obolibrary.org/obo/GAZ_00236202">
        <obo:IAO_0000115>A hydroelectric plant.</obo:IAO_0000115>
        <oboInOwl:hasOBONamespace>GAZ</oboInOwl:hasOBONamespace>
        <oboInOwl:id>GAZ:00236202</oboInOwl:id>
        <rdfs:label>Turkwel Hydro Power Plant</rdfs:label>
    </owl:NamedIndividual>
    


    <!-- http://purl.obolibrary.org/obo/GAZ_00236239 -->

    <owl:NamedIndividual rdf:about="http://purl.obolibrary.org/obo/GAZ_00236239">
        <obo:RO_0001025 rdf:resource="http://purl.obolibrary.org/obo/GAZ_00136138"/>
        <obo:IAO_0000115>A lake.</obo:IAO_0000115>
        <oboInOwl:hasOBONamespace>GAZ</oboInOwl:hasOBONamespace>
        <oboInOwl:id>GAZ:00236239</oboInOwl:id>
        <rdfs:label>Lake Kitangiri</rdfs:label>
    </owl:NamedIndividual>
    


    <!-- http://purl.obolibrary.org/obo/GAZ_00236354 -->

    <owl:NamedIndividual rdf:about="http://purl.obolibrary.org/obo/GAZ_00236354">
        <obo:RO_0001025 rdf:resource="http://purl.obolibrary.org/obo/GAZ_00015452"/>
        <obo:IAO_0000115>An island in Lake Victoria claimed by both Uganda and Kenya.</obo:IAO_0000115>
        <oboInOwl:hasOBONamespace>GAZ</oboInOwl:hasOBONamespace>
        <oboInOwl:id>GAZ:00236354</oboInOwl:id>
        <rdfs:label>Migingo Island</rdfs:label>
    </owl:NamedIndividual>
    


    <!-- http://purl.obolibrary.org/obo/GAZ_00236355 -->

    <owl:NamedIndividual rdf:about="http://purl.obolibrary.org/obo/GAZ_00236355">
        <obo:RO_0001025 rdf:resource="http://purl.obolibrary.org/obo/GAZ_00015452"/>
        <obo:IAO_0000115>A Kenyan island whose westerly most point was used to demarcate the border between Kenya and Uganda just after parallel 1 degree in Lake Victoria.</obo:IAO_0000115>
        <oboInOwl:hasOBONamespace>GAZ</oboInOwl:hasOBONamespace>
        <oboInOwl:id>GAZ:00236355</oboInOwl:id>
        <rdfs:label>Pyramid Island</rdfs:label>
    </owl:NamedIndividual>
    


    <!-- http://purl.obolibrary.org/obo/GAZ_00236356 -->

    <owl:NamedIndividual rdf:about="http://purl.obolibrary.org/obo/GAZ_00236356">
        <obo:RO_0001025 rdf:resource="http://purl.obolibrary.org/obo/GAZ_00015452"/>
        <obo:IAO_0000115>An island.</obo:IAO_0000115>
        <oboInOwl:hasOBONamespace>GAZ</oboInOwl:hasOBONamespace>
        <oboInOwl:id>GAZ:00236356</oboInOwl:id>
        <rdfs:label>Ilemba island</rdfs:label>
    </owl:NamedIndividual>
    


    <!-- http://purl.obolibrary.org/obo/GAZ_00236357 -->

    <owl:NamedIndividual rdf:about="http://purl.obolibrary.org/obo/GAZ_00236357">
        <obo:RO_0001025 rdf:resource="http://purl.obolibrary.org/obo/GAZ_00015452"/>
        <obo:IAO_0000115>An island.</obo:IAO_0000115>
        <oboInOwl:hasOBONamespace>GAZ</oboInOwl:hasOBONamespace>
        <oboInOwl:id>GAZ:00236357</oboInOwl:id>
        <rdfs:label>Sumba Island</rdfs:label>
    </owl:NamedIndividual>
    


    <!-- http://purl.obolibrary.org/obo/GAZ_00236358 -->

    <owl:NamedIndividual rdf:about="http://purl.obolibrary.org/obo/GAZ_00236358">
        <obo:RO_0001025 rdf:resource="http://purl.obolibrary.org/obo/GAZ_00015452"/>
        <obo:IAO_0000115>An island in Lake Victoria.</obo:IAO_0000115>
        <oboInOwl:hasOBONamespace>GAZ</oboInOwl:hasOBONamespace>
        <oboInOwl:id>GAZ:00236358</oboInOwl:id>
        <rdfs:label>Mageta Island</rdfs:label>
    </owl:NamedIndividual>
    


    <!-- http://purl.obolibrary.org/obo/GAZ_00236359 -->

    <owl:NamedIndividual rdf:about="http://purl.obolibrary.org/obo/GAZ_00236359">
        <obo:RO_0001025 rdf:resource="http://purl.obolibrary.org/obo/GAZ_00015452"/>
        <obo:IAO_0000115>An island.</obo:IAO_0000115>
        <oboInOwl:hasOBONamespace>GAZ</oboInOwl:hasOBONamespace>
        <oboInOwl:id>GAZ:00236359</oboInOwl:id>
        <rdfs:label>Kiringiti Island</rdfs:label>
    </owl:NamedIndividual>
    


    <!-- http://purl.obolibrary.org/obo/GAZ_00236360 -->

    <owl:NamedIndividual rdf:about="http://purl.obolibrary.org/obo/GAZ_00236360">
        <obo:RO_0001025 rdf:resource="http://purl.obolibrary.org/obo/GAZ_00015452"/>
        <obo:RO_0001025 rdf:resource="http://purl.obolibrary.org/obo/GAZ_00236658"/>
        <obo:IAO_0000115>An island.</obo:IAO_0000115>
        <oboInOwl:hasOBONamespace>GAZ</oboInOwl:hasOBONamespace>
        <oboInOwl:id>GAZ:00236360</oboInOwl:id>
        <rdfs:label>Sigulu Island</rdfs:label>
    </owl:NamedIndividual>
    


    <!-- http://purl.obolibrary.org/obo/GAZ_00236361 -->

    <owl:NamedIndividual rdf:about="http://purl.obolibrary.org/obo/GAZ_00236361">
        <obo:RO_0001025 rdf:resource="http://purl.obolibrary.org/obo/GAZ_00015452"/>
        <obo:IAO_0000115>An island.</obo:IAO_0000115>
        <oboInOwl:hasOBONamespace>GAZ</oboInOwl:hasOBONamespace>
        <oboInOwl:id>GAZ:00236361</oboInOwl:id>
        <rdfs:label>Seguti Island</rdfs:label>
    </owl:NamedIndividual>
    


    <!-- http://purl.obolibrary.org/obo/GAZ_00236362 -->

    <owl:NamedIndividual rdf:about="http://purl.obolibrary.org/obo/GAZ_00236362">
        <obo:RO_0001025 rdf:resource="http://purl.obolibrary.org/obo/GAZ_00015452"/>
        <obo:IAO_0000115>An island.</obo:IAO_0000115>
        <oboInOwl:hasOBONamespace>GAZ</oboInOwl:hasOBONamespace>
        <oboInOwl:id>GAZ:00236362</oboInOwl:id>
        <rdfs:label>Dagusi Island</rdfs:label>
    </owl:NamedIndividual>
    


    <!-- http://purl.obolibrary.org/obo/GAZ_00236363 -->

    <owl:NamedIndividual rdf:about="http://purl.obolibrary.org/obo/GAZ_00236363">
        <obo:RO_0001025 rdf:resource="http://purl.obolibrary.org/obo/GAZ_00015452"/>
        <obo:IAO_0000115>An island.</obo:IAO_0000115>
        <oboInOwl:hasOBONamespace>GAZ</oboInOwl:hasOBONamespace>
        <oboInOwl:id>GAZ:00236363</oboInOwl:id>
        <rdfs:label>Vumba Island</rdfs:label>
    </owl:NamedIndividual>
    


    <!-- http://purl.obolibrary.org/obo/GAZ_00236364 -->

    <owl:NamedIndividual rdf:about="http://purl.obolibrary.org/obo/GAZ_00236364">
        <obo:RO_0001025 rdf:resource="http://purl.obolibrary.org/obo/GAZ_00015452"/>
        <obo:IAO_0000115>An island.</obo:IAO_0000115>
        <oboInOwl:hasOBONamespace>GAZ</oboInOwl:hasOBONamespace>
        <oboInOwl:id>GAZ:00236364</oboInOwl:id>
        <rdfs:label>Kaza Island</rdfs:label>
    </owl:NamedIndividual>
    


    <!-- http://purl.obolibrary.org/obo/GAZ_00236365 -->

    <owl:NamedIndividual rdf:about="http://purl.obolibrary.org/obo/GAZ_00236365">
        <obo:RO_0001025 rdf:resource="http://purl.obolibrary.org/obo/GAZ_00015452"/>
        <obo:IAO_0000115>An island.</obo:IAO_0000115>
        <oboInOwl:hasOBONamespace>GAZ</oboInOwl:hasOBONamespace>
        <oboInOwl:id>GAZ:00236365</oboInOwl:id>
        <rdfs:label>Nambuga Island</rdfs:label>
    </owl:NamedIndividual>
    


    <!-- http://purl.obolibrary.org/obo/GAZ_00236366 -->

    <owl:NamedIndividual rdf:about="http://purl.obolibrary.org/obo/GAZ_00236366">
        <obo:RO_0001025 rdf:resource="http://purl.obolibrary.org/obo/GAZ_00015452"/>
        <obo:IAO_0000115>An island.</obo:IAO_0000115>
        <oboInOwl:hasOBONamespace>GAZ</oboInOwl:hasOBONamespace>
        <oboInOwl:id>GAZ:00236366</oboInOwl:id>
        <rdfs:label>Simu Island</rdfs:label>
    </owl:NamedIndividual>
    


    <!-- http://purl.obolibrary.org/obo/GAZ_00236367 -->

    <owl:NamedIndividual rdf:about="http://purl.obolibrary.org/obo/GAZ_00236367">
        <obo:RO_0001025 rdf:resource="http://purl.obolibrary.org/obo/GAZ_00015439"/>
        <obo:IAO_0000115>A fourth-level administrative division of Uganda.</obo:IAO_0000115>
        <oboInOwl:hasOBONamespace>GAZ</oboInOwl:hasOBONamespace>
        <oboInOwl:id>GAZ:00236367</oboInOwl:id>
        <rdfs:label>Bujumba Sub-county</rdfs:label>
    </owl:NamedIndividual>
    


    <!-- http://purl.obolibrary.org/obo/GAZ_00236368 -->

    <owl:NamedIndividual rdf:about="http://purl.obolibrary.org/obo/GAZ_00236368">
        <obo:RO_0001025 rdf:resource="http://purl.obolibrary.org/obo/GAZ_00015439"/>
        <obo:IAO_0000115>A fourth-level administrative division of Uganda.</obo:IAO_0000115>
        <oboInOwl:hasOBONamespace>GAZ</oboInOwl:hasOBONamespace>
        <oboInOwl:id>GAZ:00236368</oboInOwl:id>
        <rdfs:label>Kalangala Town</rdfs:label>
    </owl:NamedIndividual>
    


    <!-- http://purl.obolibrary.org/obo/GAZ_00236369 -->

    <owl:NamedIndividual rdf:about="http://purl.obolibrary.org/obo/GAZ_00236369">
        <obo:RO_0001025 rdf:resource="http://purl.obolibrary.org/obo/GAZ_00015439"/>
        <obo:IAO_0000115>A fourth-level administrative division of Uganda.</obo:IAO_0000115>
        <oboInOwl:hasOBONamespace>GAZ</oboInOwl:hasOBONamespace>
        <oboInOwl:id>GAZ:00236369</oboInOwl:id>
        <rdfs:label>Mugoye Sub-county</rdfs:label>
    </owl:NamedIndividual>
    


    <!-- http://purl.obolibrary.org/obo/GAZ_00236370 -->

    <owl:NamedIndividual rdf:about="http://purl.obolibrary.org/obo/GAZ_00236370">
        <obo:RO_0001025 rdf:resource="http://purl.obolibrary.org/obo/GAZ_00015440"/>
        <obo:IAO_0000115>A fourth-level administrative division of Uganda.</obo:IAO_0000115>
        <oboInOwl:hasOBONamespace>GAZ</oboInOwl:hasOBONamespace>
        <oboInOwl:id>GAZ:00236370</oboInOwl:id>
        <rdfs:label>Bubeke Sub-county</rdfs:label>
    </owl:NamedIndividual>
    


    <!-- http://purl.obolibrary.org/obo/GAZ_00236371 -->

    <owl:NamedIndividual rdf:about="http://purl.obolibrary.org/obo/GAZ_00236371">
        <obo:RO_0001025 rdf:resource="http://purl.obolibrary.org/obo/GAZ_00015440"/>
        <obo:IAO_0000115>A fourth-level administrative division of Uganda.</obo:IAO_0000115>
        <oboInOwl:hasOBONamespace>GAZ</oboInOwl:hasOBONamespace>
        <oboInOwl:id>GAZ:00236371</oboInOwl:id>
        <rdfs:label>Bufumira Sub-county</rdfs:label>
    </owl:NamedIndividual>
    


    <!-- http://purl.obolibrary.org/obo/GAZ_00236372 -->

    <owl:NamedIndividual rdf:about="http://purl.obolibrary.org/obo/GAZ_00236372">
        <obo:RO_0001025 rdf:resource="http://purl.obolibrary.org/obo/GAZ_00015440"/>
        <obo:IAO_0000115>A fourth-level administrative division of Uganda.</obo:IAO_0000115>
        <oboInOwl:hasOBONamespace>GAZ</oboInOwl:hasOBONamespace>
        <oboInOwl:id>GAZ:00236372</oboInOwl:id>
        <rdfs:label>Kyamuswa Sub-county</rdfs:label>
    </owl:NamedIndividual>
    


    <!-- http://purl.obolibrary.org/obo/GAZ_00236373 -->

    <owl:NamedIndividual rdf:about="http://purl.obolibrary.org/obo/GAZ_00236373">
        <obo:RO_0001025 rdf:resource="http://purl.obolibrary.org/obo/GAZ_00015440"/>
        <obo:IAO_0000115>A fourth-level administrative division of Uganda.</obo:IAO_0000115>
        <oboInOwl:hasOBONamespace>GAZ</oboInOwl:hasOBONamespace>
        <oboInOwl:id>GAZ:00236373</oboInOwl:id>
        <rdfs:label>Mazinga Sub-county</rdfs:label>
    </owl:NamedIndividual>
    


    <!-- http://purl.obolibrary.org/obo/GAZ_00236374 -->

    <owl:NamedIndividual rdf:about="http://purl.obolibrary.org/obo/GAZ_00236374">
        <obo:IAO_0000115>A fourth-level administrative division of Uganda.</obo:IAO_0000115>
        <oboInOwl:hasOBONamespace>GAZ</oboInOwl:hasOBONamespace>
        <oboInOwl:id>GAZ:00236374</oboInOwl:id>
        <rdfs:label>Central Division</rdfs:label>
    </owl:NamedIndividual>
    


    <!-- http://purl.obolibrary.org/obo/GAZ_00236375 -->

    <owl:NamedIndividual rdf:about="http://purl.obolibrary.org/obo/GAZ_00236375">
        <obo:RO_0001025 rdf:resource="http://purl.obolibrary.org/obo/GAZ_00236374"/>
        <obo:IAO_0000115>A fourth-level administrative division of Uganda.</obo:IAO_0000115>
        <oboInOwl:hasOBONamespace>GAZ</oboInOwl:hasOBONamespace>
        <oboInOwl:id>GAZ:00236375</oboInOwl:id>
        <rdfs:label>Kawempe Division</rdfs:label>
    </owl:NamedIndividual>
    


    <!-- http://purl.obolibrary.org/obo/GAZ_00236376 -->

    <owl:NamedIndividual rdf:about="http://purl.obolibrary.org/obo/GAZ_00236376">
        <obo:RO_0001025 rdf:resource="http://purl.obolibrary.org/obo/GAZ_00236374"/>
        <obo:IAO_0000115>A fourth-level administrative division of Uganda.</obo:IAO_0000115>
        <oboInOwl:hasOBONamespace>GAZ</oboInOwl:hasOBONamespace>
        <oboInOwl:id>GAZ:00236376</oboInOwl:id>
        <rdfs:label>Makindye Division</rdfs:label>
    </owl:NamedIndividual>
    


    <!-- http://purl.obolibrary.org/obo/GAZ_00236377 -->

    <owl:NamedIndividual rdf:about="http://purl.obolibrary.org/obo/GAZ_00236377">
        <obo:RO_0001025 rdf:resource="http://purl.obolibrary.org/obo/GAZ_00236374"/>
        <obo:IAO_0000115>A fourth-level administrative division of Uganda.</obo:IAO_0000115>
        <oboInOwl:hasOBONamespace>GAZ</oboInOwl:hasOBONamespace>
        <oboInOwl:id>GAZ:00236377</oboInOwl:id>
        <rdfs:label>Nakawa Division</rdfs:label>
    </owl:NamedIndividual>
    


    <!-- http://purl.obolibrary.org/obo/GAZ_00236378 -->

    <owl:NamedIndividual rdf:about="http://purl.obolibrary.org/obo/GAZ_00236378">
        <obo:RO_0001025 rdf:resource="http://purl.obolibrary.org/obo/GAZ_00236374"/>
        <obo:IAO_0000115>A fourth-level administrative division of Uganda.</obo:IAO_0000115>
        <oboInOwl:hasOBONamespace>GAZ</oboInOwl:hasOBONamespace>
        <oboInOwl:id>GAZ:00236378</oboInOwl:id>
        <rdfs:label>Rubaga Division</rdfs:label>
    </owl:NamedIndividual>
    


    <!-- http://purl.obolibrary.org/obo/GAZ_00236379 -->

    <owl:NamedIndividual rdf:about="http://purl.obolibrary.org/obo/GAZ_00236379">
        <obo:RO_0001025 rdf:resource="http://purl.obolibrary.org/obo/GAZ_00015442"/>
        <obo:IAO_0000115>A fourth-level administrative division of Uganda.</obo:IAO_0000115>
        <oboInOwl:hasOBONamespace>GAZ</oboInOwl:hasOBONamespace>
        <oboInOwl:id>GAZ:00236379</oboInOwl:id>
        <rdfs:label>Bbaale Sub-county</rdfs:label>
    </owl:NamedIndividual>
    


    <!-- http://purl.obolibrary.org/obo/GAZ_00236380 -->

    <owl:NamedIndividual rdf:about="http://purl.obolibrary.org/obo/GAZ_00236380">
        <obo:RO_0001025 rdf:resource="http://purl.obolibrary.org/obo/GAZ_00015442"/>
        <obo:IAO_0000115>A fourth-level administrative division of Uganda.</obo:IAO_0000115>
        <oboInOwl:hasOBONamespace>GAZ</oboInOwl:hasOBONamespace>
        <oboInOwl:id>GAZ:00236380</oboInOwl:id>
        <rdfs:label>Galiraaya Sub-county</rdfs:label>
    </owl:NamedIndividual>
    


    <!-- http://purl.obolibrary.org/obo/GAZ_00236381 -->

    <owl:NamedIndividual rdf:about="http://purl.obolibrary.org/obo/GAZ_00236381">
        <obo:RO_0001025 rdf:resource="http://purl.obolibrary.org/obo/GAZ_00015442"/>
        <obo:IAO_0000115>A fourth-level administrative division of Uganda.</obo:IAO_0000115>
        <oboInOwl:hasOBONamespace>GAZ</oboInOwl:hasOBONamespace>
        <oboInOwl:id>GAZ:00236381</oboInOwl:id>
        <rdfs:label>Kayonza Sub-county</rdfs:label>
    </owl:NamedIndividual>
    


    <!-- http://purl.obolibrary.org/obo/GAZ_00236382 -->

    <owl:NamedIndividual rdf:about="http://purl.obolibrary.org/obo/GAZ_00236382">
        <obo:RO_0001025 rdf:resource="http://purl.obolibrary.org/obo/GAZ_00015442"/>
        <obo:IAO_0000115>A fourth-level administrative division of Uganda.</obo:IAO_0000115>
        <oboInOwl:hasOBONamespace>GAZ</oboInOwl:hasOBONamespace>
        <oboInOwl:id>GAZ:00236382</oboInOwl:id>
        <rdfs:label>Wabwoko-Kitimbwa Sub-county</rdfs:label>
    </owl:NamedIndividual>
    


    <!-- http://purl.obolibrary.org/obo/GAZ_00236383 -->

    <owl:NamedIndividual rdf:about="http://purl.obolibrary.org/obo/GAZ_00236383">
        <obo:RO_0001025 rdf:resource="http://purl.obolibrary.org/obo/GAZ_00015443"/>
        <obo:IAO_0000115>A fourth-level administrative division of Uganda.</obo:IAO_0000115>
        <oboInOwl:hasOBONamespace>GAZ</oboInOwl:hasOBONamespace>
        <oboInOwl:id>GAZ:00236383</oboInOwl:id>
        <rdfs:label>Busana Sub-county</rdfs:label>
    </owl:NamedIndividual>
    


    <!-- http://purl.obolibrary.org/obo/GAZ_00236384 -->

    <owl:NamedIndividual rdf:about="http://purl.obolibrary.org/obo/GAZ_00236384">
        <obo:RO_0001025 rdf:resource="http://purl.obolibrary.org/obo/GAZ_00015443"/>
        <obo:IAO_0000115>A fourth-level administrative division of Uganda.</obo:IAO_0000115>
        <oboInOwl:hasOBONamespace>GAZ</oboInOwl:hasOBONamespace>
        <oboInOwl:id>GAZ:00236384</oboInOwl:id>
        <rdfs:label>Kangulumira Sub-County</rdfs:label>
    </owl:NamedIndividual>
    


    <!-- http://purl.obolibrary.org/obo/GAZ_00236385 -->

    <owl:NamedIndividual rdf:about="http://purl.obolibrary.org/obo/GAZ_00236385">
        <obo:RO_0001025 rdf:resource="http://purl.obolibrary.org/obo/GAZ_00015443"/>
        <obo:IAO_0000115>A fourth-level administrative division of Uganda.</obo:IAO_0000115>
        <oboInOwl:hasOBONamespace>GAZ</oboInOwl:hasOBONamespace>
        <oboInOwl:id>GAZ:00236385</oboInOwl:id>
        <rdfs:label>Kayunga Sub-county</rdfs:label>
    </owl:NamedIndividual>
    


    <!-- http://purl.obolibrary.org/obo/GAZ_00236386 -->

    <owl:NamedIndividual rdf:about="http://purl.obolibrary.org/obo/GAZ_00236386">
        <obo:RO_0001025 rdf:resource="http://purl.obolibrary.org/obo/GAZ_00015443"/>
        <obo:IAO_0000115>A fourth-level administrative division of Uganda.</obo:IAO_0000115>
        <oboInOwl:hasOBONamespace>GAZ</oboInOwl:hasOBONamespace>
        <oboInOwl:id>GAZ:00236386</oboInOwl:id>
        <rdfs:label>Kayunga Town</rdfs:label>
    </owl:NamedIndividual>
    


    <!-- http://purl.obolibrary.org/obo/GAZ_00236387 -->

    <owl:NamedIndividual rdf:about="http://purl.obolibrary.org/obo/GAZ_00236387">
        <obo:RO_0001025 rdf:resource="http://purl.obolibrary.org/obo/GAZ_00015443"/>
        <obo:IAO_0000115>A fourth-level administrative division of Uganda.</obo:IAO_0000115>
        <oboInOwl:hasOBONamespace>GAZ</oboInOwl:hasOBONamespace>
        <oboInOwl:id>GAZ:00236387</oboInOwl:id>
        <rdfs:label>Nazigo Sub-county</rdfs:label>
    </owl:NamedIndividual>
    


    <!-- http://purl.obolibrary.org/obo/GAZ_00236388 -->

    <owl:NamedIndividual rdf:about="http://purl.obolibrary.org/obo/GAZ_00236388">
        <obo:IAO_0000115>A fourth-level administrative division of Uganda.</obo:IAO_0000115>
        <oboInOwl:hasOBONamespace>GAZ</oboInOwl:hasOBONamespace>
        <oboInOwl:id>GAZ:00236388</oboInOwl:id>
        <rdfs:label>Wattuba Sub-county</rdfs:label>
    </owl:NamedIndividual>
    


    <!-- http://purl.obolibrary.org/obo/GAZ_00236389 -->

    <owl:NamedIndividual rdf:about="http://purl.obolibrary.org/obo/GAZ_00236389">
        <obo:IAO_0000115>A fourth-level administrative division of Uganda.</obo:IAO_0000115>
        <oboInOwl:hasOBONamespace>GAZ</oboInOwl:hasOBONamespace>
        <oboInOwl:id>GAZ:00236389</oboInOwl:id>
        <rdfs:label>Ntwetwe Sub-county</rdfs:label>
    </owl:NamedIndividual>
    


    <!-- http://purl.obolibrary.org/obo/GAZ_00236390 -->

    <owl:NamedIndividual rdf:about="http://purl.obolibrary.org/obo/GAZ_00236390">
        <obo:IAO_0000115>A fourth-level administrative division of Uganda.</obo:IAO_0000115>
        <oboInOwl:hasOBONamespace>GAZ</oboInOwl:hasOBONamespace>
        <oboInOwl:id>GAZ:00236390</oboInOwl:id>
        <rdfs:label>Nsambya Sub-county</rdfs:label>
    </owl:NamedIndividual>
    


    <!-- http://purl.obolibrary.org/obo/GAZ_00236391 -->

    <owl:NamedIndividual rdf:about="http://purl.obolibrary.org/obo/GAZ_00236391">
        <obo:IAO_0000115>A fourth-level administrative division of Uganda.</obo:IAO_0000115>
        <oboInOwl:hasOBONamespace>GAZ</oboInOwl:hasOBONamespace>
        <oboInOwl:id>GAZ:00236391</oboInOwl:id>
        <rdfs:label>Muwanga Sub-county</rdfs:label>
    </owl:NamedIndividual>
    


    <!-- http://purl.obolibrary.org/obo/GAZ_00236392 -->

    <owl:NamedIndividual rdf:about="http://purl.obolibrary.org/obo/GAZ_00236392">
        <obo:IAO_0000115>A fourth-level administrative division of Uganda.</obo:IAO_0000115>
        <oboInOwl:hasOBONamespace>GAZ</oboInOwl:hasOBONamespace>
        <oboInOwl:id>GAZ:00236392</oboInOwl:id>
        <rdfs:label>Bukomero Sub-county</rdfs:label>
    </owl:NamedIndividual>
    


    <!-- http://purl.obolibrary.org/obo/GAZ_00236393 -->

    <owl:NamedIndividual rdf:about="http://purl.obolibrary.org/obo/GAZ_00236393">
        <obo:IAO_0000115>A fourth-level administrative division of Uganda.</obo:IAO_0000115>
        <oboInOwl:hasOBONamespace>GAZ</oboInOwl:hasOBONamespace>
        <oboInOwl:id>GAZ:00236393</oboInOwl:id>
        <rdfs:label>Mulagi Sub-county</rdfs:label>
    </owl:NamedIndividual>
    


    <!-- http://purl.obolibrary.org/obo/GAZ_00236394 -->

    <owl:NamedIndividual rdf:about="http://purl.obolibrary.org/obo/GAZ_00236394">
        <obo:IAO_0000115>A fourth-level administrative division of Uganda.</obo:IAO_0000115>
        <oboInOwl:hasOBONamespace>GAZ</oboInOwl:hasOBONamespace>
        <oboInOwl:id>GAZ:00236394</oboInOwl:id>
        <rdfs:label>Butemba Sub-county</rdfs:label>
    </owl:NamedIndividual>
    


    <!-- http://purl.obolibrary.org/obo/GAZ_00236395 -->

    <owl:NamedIndividual rdf:about="http://purl.obolibrary.org/obo/GAZ_00236395">
        <obo:IAO_0000115>A fourth-level administrative division of Uganda.</obo:IAO_0000115>
        <oboInOwl:hasOBONamespace>GAZ</oboInOwl:hasOBONamespace>
        <oboInOwl:id>GAZ:00236395</oboInOwl:id>
        <rdfs:label>Lwamata Sub-county</rdfs:label>
    </owl:NamedIndividual>
    


    <!-- http://purl.obolibrary.org/obo/GAZ_00236396 -->

    <owl:NamedIndividual rdf:about="http://purl.obolibrary.org/obo/GAZ_00236396">
        <obo:IAO_0000115>A fourth-level administrative division of Uganda.</obo:IAO_0000115>
        <oboInOwl:hasOBONamespace>GAZ</oboInOwl:hasOBONamespace>
        <oboInOwl:id>GAZ:00236396</oboInOwl:id>
        <rdfs:label>Kyankwanzi Sub-county</rdfs:label>
    </owl:NamedIndividual>
    


    <!-- http://purl.obolibrary.org/obo/GAZ_00236397 -->

    <owl:NamedIndividual rdf:about="http://purl.obolibrary.org/obo/GAZ_00236397">
        <obo:IAO_0000115>A fourth-level administrative division of Uganda.</obo:IAO_0000115>
        <oboInOwl:hasOBONamespace>GAZ</oboInOwl:hasOBONamespace>
        <oboInOwl:id>GAZ:00236397</oboInOwl:id>
        <rdfs:label>Kiboga Town</rdfs:label>
    </owl:NamedIndividual>
    


    <!-- http://purl.obolibrary.org/obo/GAZ_00236398 -->

    <owl:NamedIndividual rdf:about="http://purl.obolibrary.org/obo/GAZ_00236398">
        <obo:IAO_0000115>A fourth-level administrative division of Uganda.</obo:IAO_0000115>
        <oboInOwl:hasOBONamespace>GAZ</oboInOwl:hasOBONamespace>
        <oboInOwl:id>GAZ:00236398</oboInOwl:id>
        <rdfs:label>Dwaniro Sub-county</rdfs:label>
    </owl:NamedIndividual>
    


    <!-- http://purl.obolibrary.org/obo/GAZ_00236399 -->

    <owl:NamedIndividual rdf:about="http://purl.obolibrary.org/obo/GAZ_00236399">
        <obo:IAO_0000115>A fourth-level administrative division of Uganda.</obo:IAO_0000115>
        <oboInOwl:hasOBONamespace>GAZ</oboInOwl:hasOBONamespace>
        <oboInOwl:id>GAZ:00236399</oboInOwl:id>
        <rdfs:label>Kibiga Sub-county</rdfs:label>
    </owl:NamedIndividual>
    


    <!-- http://purl.obolibrary.org/obo/GAZ_00236400 -->

    <owl:NamedIndividual rdf:about="http://purl.obolibrary.org/obo/GAZ_00236400">
        <obo:IAO_0000115>A fourth-level administrative division of Uganda.</obo:IAO_0000115>
        <oboInOwl:hasOBONamespace>GAZ</oboInOwl:hasOBONamespace>
        <oboInOwl:id>GAZ:00236400</oboInOwl:id>
        <rdfs:label>Gayaza Sub-county</rdfs:label>
    </owl:NamedIndividual>
    


    <!-- http://purl.obolibrary.org/obo/GAZ_00236401 -->

    <owl:NamedIndividual rdf:about="http://purl.obolibrary.org/obo/GAZ_00236401">
        <obo:IAO_0000115>A fourth-level administrative division of Uganda.</obo:IAO_0000115>
        <oboInOwl:hasOBONamespace>GAZ</oboInOwl:hasOBONamespace>
        <oboInOwl:id>GAZ:00236401</oboInOwl:id>
        <rdfs:label>Kapeke Sub-county</rdfs:label>
    </owl:NamedIndividual>
    


    <!-- http://purl.obolibrary.org/obo/GAZ_00236402 -->

    <owl:NamedIndividual rdf:about="http://purl.obolibrary.org/obo/GAZ_00236402">
        <obo:RO_0001025 rdf:resource="http://purl.obolibrary.org/obo/GAZ_00015340"/>
        <obo:IAO_0000115>A fourth-level administrative division of Uganda.</obo:IAO_0000115>
        <oboInOwl:hasOBONamespace>GAZ</oboInOwl:hasOBONamespace>
        <oboInOwl:id>GAZ:00236402</oboInOwl:id>
        <rdfs:label>Bamunanika County</rdfs:label>
    </owl:NamedIndividual>
    


    <!-- http://purl.obolibrary.org/obo/GAZ_00236404 -->

    <owl:NamedIndividual rdf:about="http://purl.obolibrary.org/obo/GAZ_00236404">
        <obo:RO_0001025 rdf:resource="http://purl.obolibrary.org/obo/GAZ_00236402"/>
        <obo:IAO_0000115>A fourth-level administrative division of Uganda.</obo:IAO_0000115>
        <oboInOwl:hasOBONamespace>GAZ</oboInOwl:hasOBONamespace>
        <oboInOwl:id>GAZ:00236404</oboInOwl:id>
        <rdfs:label>Bamunanika Sub-county</rdfs:label>
    </owl:NamedIndividual>
    


    <!-- http://purl.obolibrary.org/obo/GAZ_00236405 -->

    <owl:NamedIndividual rdf:about="http://purl.obolibrary.org/obo/GAZ_00236405">
        <obo:RO_0001025 rdf:resource="http://purl.obolibrary.org/obo/GAZ_00236402"/>
        <obo:IAO_0000115>A fourth-level administrative division of Uganda.</obo:IAO_0000115>
        <oboInOwl:hasOBONamespace>GAZ</oboInOwl:hasOBONamespace>
        <oboInOwl:id>GAZ:00236405</oboInOwl:id>
        <rdfs:label>Kalagala Sub-county</rdfs:label>
    </owl:NamedIndividual>
    


    <!-- http://purl.obolibrary.org/obo/GAZ_00236406 -->

    <owl:NamedIndividual rdf:about="http://purl.obolibrary.org/obo/GAZ_00236406">
        <obo:RO_0001025 rdf:resource="http://purl.obolibrary.org/obo/GAZ_00236402"/>
        <obo:IAO_0000115>A fourth-level administrative division of Uganda.</obo:IAO_0000115>
        <oboInOwl:hasOBONamespace>GAZ</oboInOwl:hasOBONamespace>
        <oboInOwl:id>GAZ:00236406</oboInOwl:id>
        <rdfs:label>Kamira Sub-county</rdfs:label>
    </owl:NamedIndividual>
    


    <!-- http://purl.obolibrary.org/obo/GAZ_00236407 -->

    <owl:NamedIndividual rdf:about="http://purl.obolibrary.org/obo/GAZ_00236407">
        <obo:RO_0001025 rdf:resource="http://purl.obolibrary.org/obo/GAZ_00236402"/>
        <obo:IAO_0000115>A fourth-level administrative division of Uganda.</obo:IAO_0000115>
        <oboInOwl:hasOBONamespace>GAZ</oboInOwl:hasOBONamespace>
        <oboInOwl:id>GAZ:00236407</oboInOwl:id>
        <rdfs:label>Kikyusa Sub-county</rdfs:label>
    </owl:NamedIndividual>
    


    <!-- http://purl.obolibrary.org/obo/GAZ_00236408 -->

    <owl:NamedIndividual rdf:about="http://purl.obolibrary.org/obo/GAZ_00236408">
        <obo:RO_0001025 rdf:resource="http://purl.obolibrary.org/obo/GAZ_00236402"/>
        <obo:IAO_0000115>A fourth-level administrative division of Uganda.</obo:IAO_0000115>
        <oboInOwl:hasOBONamespace>GAZ</oboInOwl:hasOBONamespace>
        <oboInOwl:id>GAZ:00236408</oboInOwl:id>
        <rdfs:label>Zirobwe Sub-county</rdfs:label>
    </owl:NamedIndividual>
    


    <!-- http://purl.obolibrary.org/obo/GAZ_00236409 -->

    <owl:NamedIndividual rdf:about="http://purl.obolibrary.org/obo/GAZ_00236409">
        <obo:RO_0001025 rdf:resource="http://purl.obolibrary.org/obo/GAZ_00015445"/>
        <obo:IAO_0000115>A fourth-level administrative division of Uganda.</obo:IAO_0000115>
        <oboInOwl:hasOBONamespace>GAZ</oboInOwl:hasOBONamespace>
        <oboInOwl:id>GAZ:00236409</oboInOwl:id>
        <rdfs:label>Bombo Town</rdfs:label>
    </owl:NamedIndividual>
    


    <!-- http://purl.obolibrary.org/obo/GAZ_00236410 -->

    <owl:NamedIndividual rdf:about="http://purl.obolibrary.org/obo/GAZ_00236410">
        <obo:RO_0001025 rdf:resource="http://purl.obolibrary.org/obo/GAZ_00015445"/>
        <obo:IAO_0000115>A fourth-level administrative division of Uganda.</obo:IAO_0000115>
        <oboInOwl:hasOBONamespace>GAZ</oboInOwl:hasOBONamespace>
        <oboInOwl:id>GAZ:00236410</oboInOwl:id>
        <rdfs:label>Butuntumula Sub-county</rdfs:label>
    </owl:NamedIndividual>
    


    <!-- http://purl.obolibrary.org/obo/GAZ_00236411 -->

    <owl:NamedIndividual rdf:about="http://purl.obolibrary.org/obo/GAZ_00236411">
        <obo:RO_0001025 rdf:resource="http://purl.obolibrary.org/obo/GAZ_00015445"/>
        <obo:IAO_0000115>A fourth-level administrative division of Uganda.</obo:IAO_0000115>
        <oboInOwl:hasOBONamespace>GAZ</oboInOwl:hasOBONamespace>
        <oboInOwl:id>GAZ:00236411</oboInOwl:id>
        <rdfs:label>Katikamu Sub-county</rdfs:label>
    </owl:NamedIndividual>
    


    <!-- http://purl.obolibrary.org/obo/GAZ_00236412 -->

    <owl:NamedIndividual rdf:about="http://purl.obolibrary.org/obo/GAZ_00236412">
        <obo:RO_0001025 rdf:resource="http://purl.obolibrary.org/obo/GAZ_00015445"/>
        <obo:IAO_0000115>A fourth-level administrative division of Uganda.</obo:IAO_0000115>
        <oboInOwl:hasOBONamespace>GAZ</oboInOwl:hasOBONamespace>
        <oboInOwl:id>GAZ:00236412</oboInOwl:id>
        <rdfs:label>Luwero Sub-county</rdfs:label>
    </owl:NamedIndividual>
    


    <!-- http://purl.obolibrary.org/obo/GAZ_00236413 -->

    <owl:NamedIndividual rdf:about="http://purl.obolibrary.org/obo/GAZ_00236413">
        <obo:RO_0001025 rdf:resource="http://purl.obolibrary.org/obo/GAZ_00015445"/>
        <obo:IAO_0000115>A fourth-level administrative division of Uganda.</obo:IAO_0000115>
        <oboInOwl:hasOBONamespace>GAZ</oboInOwl:hasOBONamespace>
        <oboInOwl:id>GAZ:00236413</oboInOwl:id>
        <rdfs:label>Luwero Town</rdfs:label>
    </owl:NamedIndividual>
    


    <!-- http://purl.obolibrary.org/obo/GAZ_00236414 -->

    <owl:NamedIndividual rdf:about="http://purl.obolibrary.org/obo/GAZ_00236414">
        <obo:RO_0001025 rdf:resource="http://purl.obolibrary.org/obo/GAZ_00015445"/>
        <obo:IAO_0000115>A fourth-level administrative division of Uganda.</obo:IAO_0000115>
        <oboInOwl:hasOBONamespace>GAZ</oboInOwl:hasOBONamespace>
        <oboInOwl:id>GAZ:00236414</oboInOwl:id>
        <rdfs:label>Makulubita Sub-county</rdfs:label>
    </owl:NamedIndividual>
    


    <!-- http://purl.obolibrary.org/obo/GAZ_00236415 -->

    <owl:NamedIndividual rdf:about="http://purl.obolibrary.org/obo/GAZ_00236415">
        <obo:RO_0001025 rdf:resource="http://purl.obolibrary.org/obo/GAZ_00015445"/>
        <obo:IAO_0000115>A fourth-level administrative division of Uganda.</obo:IAO_0000115>
        <oboInOwl:hasOBONamespace>GAZ</oboInOwl:hasOBONamespace>
        <oboInOwl:id>GAZ:00236415</oboInOwl:id>
        <rdfs:label>Nyimbwa Sub-county</rdfs:label>
    </owl:NamedIndividual>
    


    <!-- http://purl.obolibrary.org/obo/GAZ_00236416 -->

    <owl:NamedIndividual rdf:about="http://purl.obolibrary.org/obo/GAZ_00236416">
        <obo:RO_0001025 rdf:resource="http://purl.obolibrary.org/obo/GAZ_00015445"/>
        <obo:IAO_0000115>A fourth-level administrative division of Uganda.</obo:IAO_0000115>
        <oboInOwl:hasOBONamespace>GAZ</oboInOwl:hasOBONamespace>
        <oboInOwl:id>GAZ:00236416</oboInOwl:id>
        <rdfs:label>Wobulenzi Town</rdfs:label>
    </owl:NamedIndividual>
    


    <!-- http://purl.obolibrary.org/obo/GAZ_00236417 -->

    <owl:NamedIndividual rdf:about="http://purl.obolibrary.org/obo/GAZ_00236417">
        <obo:RO_0001025 rdf:resource="http://purl.obolibrary.org/obo/GAZ_00236416"/>
        <obo:IAO_0000115>A parish of Wobulenzi.</obo:IAO_0000115>
        <oboInOwl:hasOBONamespace>GAZ</oboInOwl:hasOBONamespace>
        <oboInOwl:id>GAZ:00236417</oboInOwl:id>
        <rdfs:label>Wobulenzi East Parish</rdfs:label>
    </owl:NamedIndividual>
    


    <!-- http://purl.obolibrary.org/obo/GAZ_00236418 -->

    <owl:NamedIndividual rdf:about="http://purl.obolibrary.org/obo/GAZ_00236418">
        <obo:RO_0001025 rdf:resource="http://purl.obolibrary.org/obo/GAZ_00236416"/>
        <obo:IAO_0000115>A parish of Wobulenzi.</obo:IAO_0000115>
        <oboInOwl:hasOBONamespace>GAZ</oboInOwl:hasOBONamespace>
        <oboInOwl:id>GAZ:00236418</oboInOwl:id>
        <rdfs:label>Wobulenzi West Parish</rdfs:label>
    </owl:NamedIndividual>
    


    <!-- http://purl.obolibrary.org/obo/GAZ_00236419 -->

    <owl:NamedIndividual rdf:about="http://purl.obolibrary.org/obo/GAZ_00236419">
        <obo:RO_0001025 rdf:resource="http://purl.obolibrary.org/obo/GAZ_00236416"/>
        <obo:IAO_0000115>A parish of Wobulenzi.</obo:IAO_0000115>
        <oboInOwl:hasOBONamespace>GAZ</oboInOwl:hasOBONamespace>
        <oboInOwl:id>GAZ:00236419</oboInOwl:id>
        <rdfs:label>Bukalasa Parish</rdfs:label>
    </owl:NamedIndividual>
    


    <!-- http://purl.obolibrary.org/obo/GAZ_00236420 -->

    <owl:NamedIndividual rdf:about="http://purl.obolibrary.org/obo/GAZ_00236420">
        <obo:RO_0001025 rdf:resource="http://purl.obolibrary.org/obo/GAZ_00236416"/>
        <obo:IAO_0000115>A parish of Wobulenzi.</obo:IAO_0000115>
        <oboInOwl:hasOBONamespace>GAZ</oboInOwl:hasOBONamespace>
        <oboInOwl:id>GAZ:00236420</oboInOwl:id>
        <rdfs:label>Katikamu Parish</rdfs:label>
    </owl:NamedIndividual>
    


    <!-- http://purl.obolibrary.org/obo/GAZ_00236421 -->

    <owl:NamedIndividual rdf:about="http://purl.obolibrary.org/obo/GAZ_00236421">
        <obo:RO_0001025 rdf:resource="http://purl.obolibrary.org/obo/GAZ_00236416"/>
        <obo:IAO_0000115>A parish of Wobulenzi.</obo:IAO_0000115>
        <oboInOwl:hasOBONamespace>GAZ</oboInOwl:hasOBONamespace>
        <oboInOwl:id>GAZ:00236421</oboInOwl:id>
        <rdfs:label>Wobulenzi Central Parish</rdfs:label>
    </owl:NamedIndividual>
    


    <!-- http://purl.obolibrary.org/obo/GAZ_00236422 -->

    <owl:NamedIndividual rdf:about="http://purl.obolibrary.org/obo/GAZ_00236422">
        <oboInOwl:hasOBONamespace>GAZ</oboInOwl:hasOBONamespace>
        <oboInOwl:id>GAZ:00236422</oboInOwl:id>
        <rdfs:label>Kapeeka Sub-county</rdfs:label>
    </owl:NamedIndividual>
    


    <!-- http://purl.obolibrary.org/obo/GAZ_00236423 -->

    <owl:NamedIndividual rdf:about="http://purl.obolibrary.org/obo/GAZ_00236423">
        <oboInOwl:hasOBONamespace>GAZ</oboInOwl:hasOBONamespace>
        <oboInOwl:id>GAZ:00236423</oboInOwl:id>
        <rdfs:label>Kasangombe Sub-county</rdfs:label>
    </owl:NamedIndividual>
    


    <!-- http://purl.obolibrary.org/obo/GAZ_00236424 -->

    <owl:NamedIndividual rdf:about="http://purl.obolibrary.org/obo/GAZ_00236424">
        <oboInOwl:hasOBONamespace>GAZ</oboInOwl:hasOBONamespace>
        <oboInOwl:id>GAZ:00236424</oboInOwl:id>
        <rdfs:label>Kikamulo Sub-county</rdfs:label>
    </owl:NamedIndividual>
    


    <!-- http://purl.obolibrary.org/obo/GAZ_00236425 -->

    <owl:NamedIndividual rdf:about="http://purl.obolibrary.org/obo/GAZ_00236425">
        <oboInOwl:hasOBONamespace>GAZ</oboInOwl:hasOBONamespace>
        <oboInOwl:id>GAZ:00236425</oboInOwl:id>
        <rdfs:label>Nakaseke Sub-county</rdfs:label>
    </owl:NamedIndividual>
    


    <!-- http://purl.obolibrary.org/obo/GAZ_00236426 -->

    <owl:NamedIndividual rdf:about="http://purl.obolibrary.org/obo/GAZ_00236426">
        <oboInOwl:hasOBONamespace>GAZ</oboInOwl:hasOBONamespace>
        <oboInOwl:id>GAZ:00236426</oboInOwl:id>
        <rdfs:label>Ngoma Sub-county</rdfs:label>
    </owl:NamedIndividual>
    


    <!-- http://purl.obolibrary.org/obo/GAZ_00236427 -->

    <owl:NamedIndividual rdf:about="http://purl.obolibrary.org/obo/GAZ_00236427">
        <obo:IAO_0000115>A fourth-level administrative division of Uganda.</obo:IAO_0000115>
        <oboInOwl:hasOBONamespace>GAZ</oboInOwl:hasOBONamespace>
        <oboInOwl:id>GAZ:00236427</oboInOwl:id>
        <rdfs:label>Semuto Sub-county</rdfs:label>
    </owl:NamedIndividual>
    


    <!-- http://purl.obolibrary.org/obo/GAZ_00236428 -->

    <owl:NamedIndividual rdf:about="http://purl.obolibrary.org/obo/GAZ_00236428">
        <obo:IAO_0000115>A fourth-level administrative division of Uganda.</obo:IAO_0000115>
        <oboInOwl:hasOBONamespace>GAZ</oboInOwl:hasOBONamespace>
        <oboInOwl:id>GAZ:00236428</oboInOwl:id>
        <rdfs:label>Wakyato Sub-county</rdfs:label>
    </owl:NamedIndividual>
    


    <!-- http://purl.obolibrary.org/obo/GAZ_00236429 -->

    <owl:NamedIndividual rdf:about="http://purl.obolibrary.org/obo/GAZ_00236429">
        <obo:RO_0001025 rdf:resource="http://purl.obolibrary.org/obo/GAZ_00015447"/>
        <obo:IAO_0000115>A fourth-level administrative division of Uganda.</obo:IAO_0000115>
        <oboInOwl:hasOBONamespace>GAZ</oboInOwl:hasOBONamespace>
        <oboInOwl:id>GAZ:00236429</oboInOwl:id>
        <rdfs:label>Bigasa Sub-county</rdfs:label>
    </owl:NamedIndividual>
    


    <!-- http://purl.obolibrary.org/obo/GAZ_00236430 -->

    <owl:NamedIndividual rdf:about="http://purl.obolibrary.org/obo/GAZ_00236430">
        <obo:RO_0001025 rdf:resource="http://purl.obolibrary.org/obo/GAZ_00015447"/>
        <obo:IAO_0000115>A fourth-level administrative division of Uganda.</obo:IAO_0000115>
        <oboInOwl:hasOBONamespace>GAZ</oboInOwl:hasOBONamespace>
        <oboInOwl:id>GAZ:00236430</oboInOwl:id>
        <rdfs:label>Butenga Sub-county</rdfs:label>
    </owl:NamedIndividual>
    


    <!-- http://purl.obolibrary.org/obo/GAZ_00236431 -->

    <owl:NamedIndividual rdf:about="http://purl.obolibrary.org/obo/GAZ_00236431">
        <obo:RO_0001025 rdf:resource="http://purl.obolibrary.org/obo/GAZ_00015447"/>
        <obo:IAO_0000115>A fourth-level administrative division of Uganda.</obo:IAO_0000115>
        <oboInOwl:hasOBONamespace>GAZ</oboInOwl:hasOBONamespace>
        <oboInOwl:id>GAZ:00236431</oboInOwl:id>
        <rdfs:label>Kibinge Sub-county</rdfs:label>
    </owl:NamedIndividual>
    


    <!-- http://purl.obolibrary.org/obo/GAZ_00236432 -->

    <owl:NamedIndividual rdf:about="http://purl.obolibrary.org/obo/GAZ_00236432">
        <obo:RO_0001025 rdf:resource="http://purl.obolibrary.org/obo/GAZ_00015447"/>
        <obo:IAO_0000115>A fourth-level administrative division of Uganda.</obo:IAO_0000115>
        <oboInOwl:hasOBONamespace>GAZ</oboInOwl:hasOBONamespace>
        <oboInOwl:id>GAZ:00236432</oboInOwl:id>
        <rdfs:label>Kitanda Sub-county</rdfs:label>
    </owl:NamedIndividual>
    


    <!-- http://purl.obolibrary.org/obo/GAZ_00236433 -->

    <owl:NamedIndividual rdf:about="http://purl.obolibrary.org/obo/GAZ_00236433">
        <obo:RO_0001025 rdf:resource="http://purl.obolibrary.org/obo/GAZ_00015449"/>
        <obo:IAO_0000115>A fourth-level administrative division of Uganda.</obo:IAO_0000115>
        <oboInOwl:hasOBONamespace>GAZ</oboInOwl:hasOBONamespace>
        <oboInOwl:id>GAZ:00236433</oboInOwl:id>
        <rdfs:label>Bukakata Sub-county</rdfs:label>
    </owl:NamedIndividual>
    


    <!-- http://purl.obolibrary.org/obo/GAZ_00236434 -->

    <owl:NamedIndividual rdf:about="http://purl.obolibrary.org/obo/GAZ_00236434">
        <obo:RO_0001025 rdf:resource="http://purl.obolibrary.org/obo/GAZ_00015449"/>
        <obo:IAO_0000115>A fourth-level administrative division of Uganda.</obo:IAO_0000115>
        <oboInOwl:hasOBONamespace>GAZ</oboInOwl:hasOBONamespace>
        <oboInOwl:id>GAZ:00236434</oboInOwl:id>
        <rdfs:label>Buwunga Sub-county</rdfs:label>
    </owl:NamedIndividual>
    


    <!-- http://purl.obolibrary.org/obo/GAZ_00236435 -->

    <owl:NamedIndividual rdf:about="http://purl.obolibrary.org/obo/GAZ_00236435">
        <obo:RO_0001025 rdf:resource="http://purl.obolibrary.org/obo/GAZ_00015449"/>
        <obo:IAO_0000115>A fourth-level administrative division of Uganda.</obo:IAO_0000115>
        <oboInOwl:hasOBONamespace>GAZ</oboInOwl:hasOBONamespace>
        <oboInOwl:id>GAZ:00236435</oboInOwl:id>
        <rdfs:label>Kabonera Sub-county</rdfs:label>
    </owl:NamedIndividual>
    


    <!-- http://purl.obolibrary.org/obo/GAZ_00236436 -->

    <owl:NamedIndividual rdf:about="http://purl.obolibrary.org/obo/GAZ_00236436">
        <obo:RO_0001025 rdf:resource="http://purl.obolibrary.org/obo/GAZ_00015449"/>
        <obo:IAO_0000115>A fourth-level administrative division of Uganda.</obo:IAO_0000115>
        <oboInOwl:hasOBONamespace>GAZ</oboInOwl:hasOBONamespace>
        <oboInOwl:id>GAZ:00236436</oboInOwl:id>
        <rdfs:label>Kisekka Sub-county</rdfs:label>
    </owl:NamedIndividual>
    


    <!-- http://purl.obolibrary.org/obo/GAZ_00236437 -->

    <owl:NamedIndividual rdf:about="http://purl.obolibrary.org/obo/GAZ_00236437">
        <obo:RO_0001025 rdf:resource="http://purl.obolibrary.org/obo/GAZ_00015449"/>
        <obo:IAO_0000115>A fourth-level administrative division of Uganda.</obo:IAO_0000115>
        <oboInOwl:hasOBONamespace>GAZ</oboInOwl:hasOBONamespace>
        <oboInOwl:id>GAZ:00236437</oboInOwl:id>
        <rdfs:label>Kkingo Sub-county</rdfs:label>
    </owl:NamedIndividual>
    


    <!-- http://purl.obolibrary.org/obo/GAZ_00236438 -->

    <owl:NamedIndividual rdf:about="http://purl.obolibrary.org/obo/GAZ_00236438">
        <obo:RO_0001025 rdf:resource="http://purl.obolibrary.org/obo/GAZ_00015449"/>
        <obo:IAO_0000115>A fourth-level administrative division of Uganda.</obo:IAO_0000115>
        <oboInOwl:hasOBONamespace>GAZ</oboInOwl:hasOBONamespace>
        <oboInOwl:id>GAZ:00236438</oboInOwl:id>
        <rdfs:label>Kyanamukaaka Sub-county</rdfs:label>
    </owl:NamedIndividual>
    


    <!-- http://purl.obolibrary.org/obo/GAZ_00236439 -->

    <owl:NamedIndividual rdf:about="http://purl.obolibrary.org/obo/GAZ_00236439">
        <obo:RO_0001025 rdf:resource="http://purl.obolibrary.org/obo/GAZ_00015449"/>
        <obo:IAO_0000115>A fourth-level administrative division of Uganda.</obo:IAO_0000115>
        <oboInOwl:hasOBONamespace>GAZ</oboInOwl:hasOBONamespace>
        <oboInOwl:id>GAZ:00236439</oboInOwl:id>
        <rdfs:label>Kyazanga Sub-county</rdfs:label>
    </owl:NamedIndividual>
    


    <!-- http://purl.obolibrary.org/obo/GAZ_00236440 -->

    <owl:NamedIndividual rdf:about="http://purl.obolibrary.org/obo/GAZ_00236440">
        <obo:RO_0001025 rdf:resource="http://purl.obolibrary.org/obo/GAZ_00015449"/>
        <obo:IAO_0000115>A fourth-level administrative division of Uganda.</obo:IAO_0000115>
        <oboInOwl:hasOBONamespace>GAZ</oboInOwl:hasOBONamespace>
        <oboInOwl:id>GAZ:00236440</oboInOwl:id>
        <rdfs:label>Lwengo Sub-county</rdfs:label>
    </owl:NamedIndividual>
    


    <!-- http://purl.obolibrary.org/obo/GAZ_00236441 -->

    <owl:NamedIndividual rdf:about="http://purl.obolibrary.org/obo/GAZ_00236441">
        <obo:RO_0001025 rdf:resource="http://purl.obolibrary.org/obo/GAZ_00015449"/>
        <obo:IAO_0000115>A fourth-level administrative division of Uganda.</obo:IAO_0000115>
        <oboInOwl:hasOBONamespace>GAZ</oboInOwl:hasOBONamespace>
        <oboInOwl:id>GAZ:00236441</oboInOwl:id>
        <rdfs:label>Malongo Sub-county</rdfs:label>
    </owl:NamedIndividual>
    


    <!-- http://purl.obolibrary.org/obo/GAZ_00236442 -->

    <owl:NamedIndividual rdf:about="http://purl.obolibrary.org/obo/GAZ_00236442">
        <obo:RO_0001025 rdf:resource="http://purl.obolibrary.org/obo/GAZ_00015449"/>
        <obo:IAO_0000115>A fourth-level administrative division of Uganda.</obo:IAO_0000115>
        <oboInOwl:hasOBONamespace>GAZ</oboInOwl:hasOBONamespace>
        <oboInOwl:id>GAZ:00236442</oboInOwl:id>
        <rdfs:label>Mukungwe Sub-county</rdfs:label>
    </owl:NamedIndividual>
    


    <!-- http://purl.obolibrary.org/obo/GAZ_00236443 -->

    <owl:NamedIndividual rdf:about="http://purl.obolibrary.org/obo/GAZ_00236443">
        <obo:RO_0001025 rdf:resource="http://purl.obolibrary.org/obo/GAZ_00015449"/>
        <obo:IAO_0000115>A fourth-level administrative division of Uganda.</obo:IAO_0000115>
        <oboInOwl:hasOBONamespace>GAZ</oboInOwl:hasOBONamespace>
        <oboInOwl:id>GAZ:00236443</oboInOwl:id>
        <rdfs:label>Ndagwe Sub-county</rdfs:label>
    </owl:NamedIndividual>
    


    <!-- http://purl.obolibrary.org/obo/GAZ_00236444 -->

    <owl:NamedIndividual rdf:about="http://purl.obolibrary.org/obo/GAZ_00236444">
        <obo:RO_0001025 rdf:resource="http://purl.obolibrary.org/obo/GAZ_00015448"/>
        <obo:IAO_0000115>A fourth-level administrative division of Uganda.</obo:IAO_0000115>
        <oboInOwl:hasOBONamespace>GAZ</oboInOwl:hasOBONamespace>
        <oboInOwl:id>GAZ:00236444</oboInOwl:id>
        <rdfs:label>Bukulula Sub-county</rdfs:label>
    </owl:NamedIndividual>
    


    <!-- http://purl.obolibrary.org/obo/GAZ_00236445 -->

    <owl:NamedIndividual rdf:about="http://purl.obolibrary.org/obo/GAZ_00236445">
        <obo:RO_0001025 rdf:resource="http://purl.obolibrary.org/obo/GAZ_00015448"/>
        <obo:IAO_0000115>A fourth-level administrative division of Uganda.</obo:IAO_0000115>
        <oboInOwl:hasOBONamespace>GAZ</oboInOwl:hasOBONamespace>
        <oboInOwl:id>GAZ:00236445</oboInOwl:id>
        <rdfs:label>Kalungu Sub-county</rdfs:label>
    </owl:NamedIndividual>
    


    <!-- http://purl.obolibrary.org/obo/GAZ_00236446 -->

    <owl:NamedIndividual rdf:about="http://purl.obolibrary.org/obo/GAZ_00236446">
        <obo:RO_0001025 rdf:resource="http://purl.obolibrary.org/obo/GAZ_00015448"/>
        <obo:IAO_0000115>A fourth-level administrative division of Uganda.</obo:IAO_0000115>
        <oboInOwl:hasOBONamespace>GAZ</oboInOwl:hasOBONamespace>
        <oboInOwl:id>GAZ:00236446</oboInOwl:id>
        <rdfs:label>Kyamuliibwa Sub-county</rdfs:label>
    </owl:NamedIndividual>
    


    <!-- http://purl.obolibrary.org/obo/GAZ_00236447 -->

    <owl:NamedIndividual rdf:about="http://purl.obolibrary.org/obo/GAZ_00236447">
        <obo:RO_0001025 rdf:resource="http://purl.obolibrary.org/obo/GAZ_00015448"/>
        <obo:IAO_0000115>A fourth-level administrative division of Uganda.</obo:IAO_0000115>
        <oboInOwl:hasOBONamespace>GAZ</oboInOwl:hasOBONamespace>
        <oboInOwl:id>GAZ:00236447</oboInOwl:id>
        <rdfs:label>Lukaya Town</rdfs:label>
    </owl:NamedIndividual>
    


    <!-- http://purl.obolibrary.org/obo/GAZ_00236448 -->

    <owl:NamedIndividual rdf:about="http://purl.obolibrary.org/obo/GAZ_00236448">
        <obo:RO_0001025 rdf:resource="http://purl.obolibrary.org/obo/GAZ_00015448"/>
        <obo:IAO_0000115>A fourth-level administrative division of Uganda.</obo:IAO_0000115>
        <oboInOwl:hasOBONamespace>GAZ</oboInOwl:hasOBONamespace>
        <oboInOwl:id>GAZ:00236448</oboInOwl:id>
        <rdfs:label>Lwabenge Sub-county</rdfs:label>
    </owl:NamedIndividual>
    


    <!-- http://purl.obolibrary.org/obo/GAZ_00236449 -->

    <owl:NamedIndividual rdf:about="http://purl.obolibrary.org/obo/GAZ_00236449">
        <obo:RO_0001025 rdf:resource="http://purl.obolibrary.org/obo/GAZ_00012976"/>
        <obo:IAO_0000115>A fourth-level administrative division of Uganda.</obo:IAO_0000115>
        <oboInOwl:hasOBONamespace>GAZ</oboInOwl:hasOBONamespace>
        <oboInOwl:id>GAZ:00236449</oboInOwl:id>
        <rdfs:label>Katwe/Butego Sub-county</rdfs:label>
    </owl:NamedIndividual>
    


    <!-- http://purl.obolibrary.org/obo/GAZ_00236450 -->

    <owl:NamedIndividual rdf:about="http://purl.obolibrary.org/obo/GAZ_00236450">
        <obo:RO_0001025 rdf:resource="http://purl.obolibrary.org/obo/GAZ_00012976"/>
        <obo:IAO_0000115>A fourth-level administrative division of Uganda.</obo:IAO_0000115>
        <oboInOwl:hasOBONamespace>GAZ</oboInOwl:hasOBONamespace>
        <oboInOwl:id>GAZ:00236450</oboInOwl:id>
        <rdfs:label>Kimanya/Kyabakuza Sub-county</rdfs:label>
    </owl:NamedIndividual>
    


    <!-- http://purl.obolibrary.org/obo/GAZ_00236451 -->

    <owl:NamedIndividual rdf:about="http://purl.obolibrary.org/obo/GAZ_00236451">
        <obo:RO_0001025 rdf:resource="http://purl.obolibrary.org/obo/GAZ_00012976"/>
        <obo:IAO_0000115>A fourth-level administrative division of Uganda.</obo:IAO_0000115>
        <oboInOwl:hasOBONamespace>GAZ</oboInOwl:hasOBONamespace>
        <oboInOwl:id>GAZ:00236451</oboInOwl:id>
        <rdfs:label>Nyendo/Senyange Sub-county</rdfs:label>
    </owl:NamedIndividual>
    


    <!-- http://purl.obolibrary.org/obo/GAZ_00236452 -->

    <owl:NamedIndividual rdf:about="http://purl.obolibrary.org/obo/GAZ_00236452">
        <obo:RO_0001025 rdf:resource="http://purl.obolibrary.org/obo/GAZ_00012976"/>
        <obo:IAO_0000115>A freshwater lake in Uganda. It is separated from Lake Victoria by a sand bar. A Ramsar Site.</obo:IAO_0000115>
        <oboInOwl:hasOBONamespace>GAZ</oboInOwl:hasOBONamespace>
        <oboInOwl:id>GAZ:00236452</oboInOwl:id>
        <rdfs:label>Lake Nabugabo</rdfs:label>
    </owl:NamedIndividual>
    


    <!-- http://purl.obolibrary.org/obo/GAZ_00236454 -->

    <owl:NamedIndividual rdf:about="http://purl.obolibrary.org/obo/GAZ_00236454">
        <obo:RO_0001025 rdf:resource="http://purl.obolibrary.org/obo/GAZ_00015450"/>
        <obo:IAO_0000115>A fourth-level administrative division of Uganda.</obo:IAO_0000115>
        <oboInOwl:hasOBONamespace>GAZ</oboInOwl:hasOBONamespace>
        <oboInOwl:id>GAZ:00236454</oboInOwl:id>
        <rdfs:label>Butayunja Sub-county</rdfs:label>
    </owl:NamedIndividual>
    


    <!-- http://purl.obolibrary.org/obo/GAZ_00236455 -->

    <owl:NamedIndividual rdf:about="http://purl.obolibrary.org/obo/GAZ_00236455">
        <obo:RO_0001025 rdf:resource="http://purl.obolibrary.org/obo/GAZ_00015450"/>
        <obo:IAO_0000115>A fourth-level administrative division of Uganda.</obo:IAO_0000115>
        <oboInOwl:hasOBONamespace>GAZ</oboInOwl:hasOBONamespace>
        <oboInOwl:id>GAZ:00236455</oboInOwl:id>
        <rdfs:label>Kakindu Sub-county</rdfs:label>
    </owl:NamedIndividual>
    


    <!-- http://purl.obolibrary.org/obo/GAZ_00236456 -->

    <owl:NamedIndividual rdf:about="http://purl.obolibrary.org/obo/GAZ_00236456">
        <obo:RO_0001025 rdf:resource="http://purl.obolibrary.org/obo/GAZ_00015450"/>
        <obo:IAO_0000115>A fourth-level administrative division of Uganda.</obo:IAO_0000115>
        <oboInOwl:hasOBONamespace>GAZ</oboInOwl:hasOBONamespace>
        <oboInOwl:id>GAZ:00236456</oboInOwl:id>
        <rdfs:label>Kakindu Sub-county</rdfs:label>
    </owl:NamedIndividual>
    


    <!-- http://purl.obolibrary.org/obo/GAZ_00236457 -->

    <owl:NamedIndividual rdf:about="http://purl.obolibrary.org/obo/GAZ_00236457">
        <obo:RO_0001025 rdf:resource="http://purl.obolibrary.org/obo/GAZ_00015450"/>
        <obo:IAO_0000115>A fourth-level administrative division of Uganda.</obo:IAO_0000115>
        <oboInOwl:hasOBONamespace>GAZ</oboInOwl:hasOBONamespace>
        <oboInOwl:id>GAZ:00236457</oboInOwl:id>
        <rdfs:label>Maanyi Sub-county</rdfs:label>
    </owl:NamedIndividual>
    


    <!-- http://purl.obolibrary.org/obo/GAZ_00236458 -->

    <owl:NamedIndividual rdf:about="http://purl.obolibrary.org/obo/GAZ_00236458">
        <obo:RO_0001025 rdf:resource="http://purl.obolibrary.org/obo/GAZ_00015450"/>
        <obo:IAO_0000115>A fourth-level administrative division of Uganda.</obo:IAO_0000115>
        <oboInOwl:hasOBONamespace>GAZ</oboInOwl:hasOBONamespace>
        <oboInOwl:id>GAZ:00236458</oboInOwl:id>
        <rdfs:label>Malangala Sub-county</rdfs:label>
    </owl:NamedIndividual>
    


    <!-- http://purl.obolibrary.org/obo/GAZ_00236459 -->

    <owl:NamedIndividual rdf:about="http://purl.obolibrary.org/obo/GAZ_00236459">
        <obo:RO_0001025 rdf:resource="http://purl.obolibrary.org/obo/GAZ_00015451"/>
        <obo:IAO_0000115>A fourth-level administrative division of Uganda.</obo:IAO_0000115>
        <oboInOwl:hasOBONamespace>GAZ</oboInOwl:hasOBONamespace>
        <oboInOwl:id>GAZ:00236459</oboInOwl:id>
        <rdfs:label>Bulera Sub-county</rdfs:label>
    </owl:NamedIndividual>
    


    <!-- http://purl.obolibrary.org/obo/GAZ_00236460 -->

    <owl:NamedIndividual rdf:about="http://purl.obolibrary.org/obo/GAZ_00236460">
        <obo:RO_0001025 rdf:resource="http://purl.obolibrary.org/obo/GAZ_00015451"/>
        <obo:IAO_0000115>A fourth-level administrative division of Uganda.</obo:IAO_0000115>
        <oboInOwl:hasOBONamespace>GAZ</oboInOwl:hasOBONamespace>
        <oboInOwl:id>GAZ:00236460</oboInOwl:id>
        <rdfs:label>Busimbi Sub-county</rdfs:label>
    </owl:NamedIndividual>
    


    <!-- http://purl.obolibrary.org/obo/GAZ_00236461 -->

    <owl:NamedIndividual rdf:about="http://purl.obolibrary.org/obo/GAZ_00236461">
        <obo:RO_0001025 rdf:resource="http://purl.obolibrary.org/obo/GAZ_00015451"/>
        <obo:IAO_0000115>A fourth-level administrative division of Uganda.</obo:IAO_0000115>
        <oboInOwl:hasOBONamespace>GAZ</oboInOwl:hasOBONamespace>
        <oboInOwl:id>GAZ:00236461</oboInOwl:id>
        <rdfs:label>Kikandwa Sub-county</rdfs:label>
    </owl:NamedIndividual>
    


    <!-- http://purl.obolibrary.org/obo/GAZ_00236462 -->

    <owl:NamedIndividual rdf:about="http://purl.obolibrary.org/obo/GAZ_00236462">
        <obo:RO_0001025 rdf:resource="http://purl.obolibrary.org/obo/GAZ_00015451"/>
        <obo:IAO_0000115>A fourth-level administrative division of Uganda.</obo:IAO_0000115>
        <oboInOwl:hasOBONamespace>GAZ</oboInOwl:hasOBONamespace>
        <oboInOwl:id>GAZ:00236462</oboInOwl:id>
        <rdfs:label>Mityana Town</rdfs:label>
    </owl:NamedIndividual>
    


    <!-- http://purl.obolibrary.org/obo/GAZ_00236463 -->

    <owl:NamedIndividual rdf:about="http://purl.obolibrary.org/obo/GAZ_00236463">
        <obo:RO_0001025 rdf:resource="http://purl.obolibrary.org/obo/GAZ_00015451"/>
        <obo:IAO_0000115>A fourth-level administrative division of Uganda.</obo:IAO_0000115>
        <oboInOwl:hasOBONamespace>GAZ</oboInOwl:hasOBONamespace>
        <oboInOwl:id>GAZ:00236463</oboInOwl:id>
        <rdfs:label>Ssekanyonyi Sub-county</rdfs:label>
    </owl:NamedIndividual>
    


    <!-- http://purl.obolibrary.org/obo/GAZ_00236465 -->

    <owl:NamedIndividual rdf:about="http://purl.obolibrary.org/obo/GAZ_00236465">
        <obo:IAO_0000115>An island.</obo:IAO_0000115>
        <oboInOwl:hasOBONamespace>GAZ</oboInOwl:hasOBONamespace>
        <oboInOwl:id>GAZ:00236465</oboInOwl:id>
        <rdfs:label>Lwanja Island</rdfs:label>
    </owl:NamedIndividual>
    


    <!-- http://purl.obolibrary.org/obo/GAZ_00236466 -->

    <owl:NamedIndividual rdf:about="http://purl.obolibrary.org/obo/GAZ_00236466">
        <obo:IAO_0000115>An island.</obo:IAO_0000115>
        <oboInOwl:hasOBONamespace>GAZ</oboInOwl:hasOBONamespace>
        <oboInOwl:id>GAZ:00236466</oboInOwl:id>
        <rdfs:label>Mabo Island</rdfs:label>
    </owl:NamedIndividual>
    


    <!-- http://purl.obolibrary.org/obo/GAZ_00236467 -->

    <owl:NamedIndividual rdf:about="http://purl.obolibrary.org/obo/GAZ_00236467">
        <obo:IAO_0000115>An island.</obo:IAO_0000115>
        <oboInOwl:hasOBONamespace>GAZ</oboInOwl:hasOBONamespace>
        <oboInOwl:id>GAZ:00236467</oboInOwl:id>
        <rdfs:label>Bagwe Island</rdfs:label>
    </owl:NamedIndividual>
    


    <!-- http://purl.obolibrary.org/obo/GAZ_00236475 -->

    <owl:NamedIndividual rdf:about="http://purl.obolibrary.org/obo/GAZ_00236475">
        <obo:RO_0001025 rdf:resource="http://purl.obolibrary.org/obo/GAZ_00015403"/>
        <obo:IAO_0000115>A protected area of forest-fringed wetlands along the Katonga River.</obo:IAO_0000115>
        <oboInOwl:hasOBONamespace>GAZ</oboInOwl:hasOBONamespace>
        <oboInOwl:id>GAZ:00236475</oboInOwl:id>
        <rdfs:label>Katonga Wildlife Reserve</rdfs:label>
    </owl:NamedIndividual>
    


    <!-- http://purl.obolibrary.org/obo/GAZ_00236476 -->

    <owl:NamedIndividual rdf:about="http://purl.obolibrary.org/obo/GAZ_00236476">
        <obo:RO_0001025 rdf:resource="http://purl.obolibrary.org/obo/GAZ_00015436"/>
        <obo:IAO_0000115>A fourth-level administrative division of Uganda.</obo:IAO_0000115>
        <oboInOwl:hasOBONamespace>GAZ</oboInOwl:hasOBONamespace>
        <oboInOwl:id>GAZ:00236476</oboInOwl:id>
        <rdfs:label>Budde Sub-County</rdfs:label>
    </owl:NamedIndividual>
    


    <!-- http://purl.obolibrary.org/obo/GAZ_00236477 -->

    <owl:NamedIndividual rdf:about="http://purl.obolibrary.org/obo/GAZ_00236477">
        <obo:RO_0001025 rdf:resource="http://purl.obolibrary.org/obo/GAZ_00015436"/>
        <obo:IAO_0000115>A fourth-level administrative division of Uganda.</obo:IAO_0000115>
        <oboInOwl:hasOBONamespace>GAZ</oboInOwl:hasOBONamespace>
        <oboInOwl:id>GAZ:00236477</oboInOwl:id>
        <rdfs:label>Bulo Sub-County</rdfs:label>
    </owl:NamedIndividual>
    


    <!-- http://purl.obolibrary.org/obo/GAZ_00236478 -->

    <owl:NamedIndividual rdf:about="http://purl.obolibrary.org/obo/GAZ_00236478">
        <obo:RO_0001025 rdf:resource="http://purl.obolibrary.org/obo/GAZ_00015436"/>
        <obo:IAO_0000115>A fourth-level administrative division of Uganda.</obo:IAO_0000115>
        <oboInOwl:hasOBONamespace>GAZ</oboInOwl:hasOBONamespace>
        <oboInOwl:id>GAZ:00236478</oboInOwl:id>
        <rdfs:label>Kalamba Sub-County</rdfs:label>
    </owl:NamedIndividual>
    


    <!-- http://purl.obolibrary.org/obo/GAZ_00236479 -->

    <owl:NamedIndividual rdf:about="http://purl.obolibrary.org/obo/GAZ_00236479">
        <obo:RO_0001025 rdf:resource="http://purl.obolibrary.org/obo/GAZ_00015436"/>
        <obo:IAO_0000115>A fourth-level administrative division of Uganda.</obo:IAO_0000115>
        <oboInOwl:hasOBONamespace>GAZ</oboInOwl:hasOBONamespace>
        <oboInOwl:id>GAZ:00236479</oboInOwl:id>
        <rdfs:label>Kibibi Sub-County</rdfs:label>
    </owl:NamedIndividual>
    


    <!-- http://purl.obolibrary.org/obo/GAZ_00236480 -->

    <owl:NamedIndividual rdf:about="http://purl.obolibrary.org/obo/GAZ_00236480">
        <obo:RO_0001025 rdf:resource="http://purl.obolibrary.org/obo/GAZ_00015436"/>
        <obo:IAO_0000115>A fourth-level administrative division of Uganda.</obo:IAO_0000115>
        <oboInOwl:hasOBONamespace>GAZ</oboInOwl:hasOBONamespace>
        <oboInOwl:id>GAZ:00236480</oboInOwl:id>
        <rdfs:label>Ngando Sub-County</rdfs:label>
    </owl:NamedIndividual>
    


    <!-- http://purl.obolibrary.org/obo/GAZ_00236481 -->

    <owl:NamedIndividual rdf:about="http://purl.obolibrary.org/obo/GAZ_00236481">
        <obo:RO_0001025 rdf:resource="http://purl.obolibrary.org/obo/GAZ_00015438"/>
        <obo:IAO_0000115>A fourth-level administrative division of Uganda.</obo:IAO_0000115>
        <oboInOwl:hasOBONamespace>GAZ</oboInOwl:hasOBONamespace>
        <oboInOwl:id>GAZ:00236481</oboInOwl:id>
        <rdfs:label>Kabulasoke Sub-county</rdfs:label>
    </owl:NamedIndividual>
    


    <!-- http://purl.obolibrary.org/obo/GAZ_00236482 -->

    <owl:NamedIndividual rdf:about="http://purl.obolibrary.org/obo/GAZ_00236482">
        <obo:RO_0001025 rdf:resource="http://purl.obolibrary.org/obo/GAZ_00015438"/>
        <obo:IAO_0000115>A fourth-level administrative division of Uganda.</obo:IAO_0000115>
        <oboInOwl:hasOBONamespace>GAZ</oboInOwl:hasOBONamespace>
        <oboInOwl:id>GAZ:00236482</oboInOwl:id>
        <rdfs:label>Kyegonza Sub-county</rdfs:label>
    </owl:NamedIndividual>
    


    <!-- http://purl.obolibrary.org/obo/GAZ_00236483 -->

    <owl:NamedIndividual rdf:about="http://purl.obolibrary.org/obo/GAZ_00236483">
        <obo:RO_0001025 rdf:resource="http://purl.obolibrary.org/obo/GAZ_00015438"/>
        <obo:IAO_0000115>A fourth-level administrative division of Uganda.</obo:IAO_0000115>
        <oboInOwl:hasOBONamespace>GAZ</oboInOwl:hasOBONamespace>
        <oboInOwl:id>GAZ:00236483</oboInOwl:id>
        <rdfs:label>Maddu Sub-county</rdfs:label>
    </owl:NamedIndividual>
    


    <!-- http://purl.obolibrary.org/obo/GAZ_00236484 -->

    <owl:NamedIndividual rdf:about="http://purl.obolibrary.org/obo/GAZ_00236484">
        <obo:RO_0001025 rdf:resource="http://purl.obolibrary.org/obo/GAZ_00015438"/>
        <obo:IAO_0000115>A fourth-level administrative division of Uganda.</obo:IAO_0000115>
        <oboInOwl:hasOBONamespace>GAZ</oboInOwl:hasOBONamespace>
        <oboInOwl:id>GAZ:00236484</oboInOwl:id>
        <rdfs:label>Mpenja Sub-county</rdfs:label>
    </owl:NamedIndividual>
    


    <!-- http://purl.obolibrary.org/obo/GAZ_00236485 -->

    <owl:NamedIndividual rdf:about="http://purl.obolibrary.org/obo/GAZ_00236485">
        <obo:RO_0001025 rdf:resource="http://purl.obolibrary.org/obo/GAZ_00015437"/>
        <obo:IAO_0000115>A fourth-level administrative division of Uganda.</obo:IAO_0000115>
        <oboInOwl:hasOBONamespace>GAZ</oboInOwl:hasOBONamespace>
        <oboInOwl:id>GAZ:00236485</oboInOwl:id>
        <rdfs:label>Buwama Sub-county</rdfs:label>
    </owl:NamedIndividual>
    


    <!-- http://purl.obolibrary.org/obo/GAZ_00236486 -->

    <owl:NamedIndividual rdf:about="http://purl.obolibrary.org/obo/GAZ_00236486">
        <obo:RO_0001025 rdf:resource="http://purl.obolibrary.org/obo/GAZ_00015437"/>
        <obo:IAO_0000115>A fourth-level administrative division of Uganda.</obo:IAO_0000115>
        <oboInOwl:hasOBONamespace>GAZ</oboInOwl:hasOBONamespace>
        <oboInOwl:id>GAZ:00236486</oboInOwl:id>
        <rdfs:label>Kamengo Sub-county</rdfs:label>
    </owl:NamedIndividual>
    


    <!-- http://purl.obolibrary.org/obo/GAZ_00236487 -->

    <owl:NamedIndividual rdf:about="http://purl.obolibrary.org/obo/GAZ_00236487">
        <obo:RO_0001025 rdf:resource="http://purl.obolibrary.org/obo/GAZ_00015437"/>
        <obo:IAO_0000115>A fourth-level administrative division of Uganda.</obo:IAO_0000115>
        <oboInOwl:hasOBONamespace>GAZ</oboInOwl:hasOBONamespace>
        <oboInOwl:id>GAZ:00236487</oboInOwl:id>
        <rdfs:label>Kiringente Sub-county</rdfs:label>
    </owl:NamedIndividual>
    


    <!-- http://purl.obolibrary.org/obo/GAZ_00236488 -->

    <owl:NamedIndividual rdf:about="http://purl.obolibrary.org/obo/GAZ_00236488">
        <obo:RO_0001025 rdf:resource="http://purl.obolibrary.org/obo/GAZ_00015437"/>
        <obo:IAO_0000115>A fourth-level administrative division of Uganda.</obo:IAO_0000115>
        <oboInOwl:hasOBONamespace>GAZ</oboInOwl:hasOBONamespace>
        <oboInOwl:id>GAZ:00236488</oboInOwl:id>
        <rdfs:label>Kituntu Sub-county</rdfs:label>
    </owl:NamedIndividual>
    


    <!-- http://purl.obolibrary.org/obo/GAZ_00236489 -->

    <owl:NamedIndividual rdf:about="http://purl.obolibrary.org/obo/GAZ_00236489">
        <obo:RO_0001025 rdf:resource="http://purl.obolibrary.org/obo/GAZ_00015437"/>
        <obo:IAO_0000115>A fourth-level administrative division of Uganda.</obo:IAO_0000115>
        <oboInOwl:hasOBONamespace>GAZ</oboInOwl:hasOBONamespace>
        <oboInOwl:id>GAZ:00236489</oboInOwl:id>
        <rdfs:label>Mpigi Sub-county</rdfs:label>
    </owl:NamedIndividual>
    


    <!-- http://purl.obolibrary.org/obo/GAZ_00236490 -->

    <owl:NamedIndividual rdf:about="http://purl.obolibrary.org/obo/GAZ_00236490">
        <obo:RO_0001025 rdf:resource="http://purl.obolibrary.org/obo/GAZ_00015437"/>
        <obo:IAO_0000115>A fourth-level administrative division of Uganda.</obo:IAO_0000115>
        <oboInOwl:hasOBONamespace>GAZ</oboInOwl:hasOBONamespace>
        <oboInOwl:id>GAZ:00236490</oboInOwl:id>
        <rdfs:label>Mpigi Town</rdfs:label>
    </owl:NamedIndividual>
    


    <!-- http://purl.obolibrary.org/obo/GAZ_00236491 -->

    <owl:NamedIndividual rdf:about="http://purl.obolibrary.org/obo/GAZ_00236491">
        <obo:RO_0001025 rdf:resource="http://purl.obolibrary.org/obo/GAZ_00015437"/>
        <obo:IAO_0000115>A fourth-level administrative division of Uganda.</obo:IAO_0000115>
        <oboInOwl:hasOBONamespace>GAZ</oboInOwl:hasOBONamespace>
        <oboInOwl:id>GAZ:00236491</oboInOwl:id>
        <rdfs:label>Muduma Sub-county</rdfs:label>
    </owl:NamedIndividual>
    


    <!-- http://purl.obolibrary.org/obo/GAZ_00236492 -->

    <owl:NamedIndividual rdf:about="http://purl.obolibrary.org/obo/GAZ_00236492">
        <obo:RO_0001025 rdf:resource="http://purl.obolibrary.org/obo/GAZ_00015437"/>
        <obo:IAO_0000115>A fourth-level administrative division of Uganda.</obo:IAO_0000115>
        <oboInOwl:hasOBONamespace>GAZ</oboInOwl:hasOBONamespace>
        <oboInOwl:id>GAZ:00236492</oboInOwl:id>
        <rdfs:label>Nkozi Sub-county</rdfs:label>
    </owl:NamedIndividual>
    


    <!-- http://purl.obolibrary.org/obo/GAZ_00236493 -->

    <owl:NamedIndividual rdf:about="http://purl.obolibrary.org/obo/GAZ_00236493">
        <obo:RO_0001025 rdf:resource="http://purl.obolibrary.org/obo/GAZ_00015435"/>
        <obo:IAO_0000115>A fourth-level administrative division of Uganda.</obo:IAO_0000115>
        <oboInOwl:hasOBONamespace>GAZ</oboInOwl:hasOBONamespace>
        <oboInOwl:id>GAZ:00236493</oboInOwl:id>
        <rdfs:label>Bukuya Sub-county</rdfs:label>
    </owl:NamedIndividual>
    


    <!-- http://purl.obolibrary.org/obo/GAZ_00236494 -->

    <owl:NamedIndividual rdf:about="http://purl.obolibrary.org/obo/GAZ_00236494">
        <obo:RO_0001025 rdf:resource="http://purl.obolibrary.org/obo/GAZ_00015435"/>
        <obo:IAO_0000115>A fourth-level administrative division of Uganda.</obo:IAO_0000115>
        <oboInOwl:hasOBONamespace>GAZ</oboInOwl:hasOBONamespace>
        <oboInOwl:id>GAZ:00236494</oboInOwl:id>
        <rdfs:label>Kassanda Sub-county</rdfs:label>
    </owl:NamedIndividual>
    


    <!-- http://purl.obolibrary.org/obo/GAZ_00236495 -->

    <owl:NamedIndividual rdf:about="http://purl.obolibrary.org/obo/GAZ_00236495">
        <obo:RO_0001025 rdf:resource="http://purl.obolibrary.org/obo/GAZ_00015435"/>
        <obo:IAO_0000115>A fourth-level administrative division of Uganda.</obo:IAO_0000115>
        <oboInOwl:hasOBONamespace>GAZ</oboInOwl:hasOBONamespace>
        <oboInOwl:id>GAZ:00236495</oboInOwl:id>
        <rdfs:label>Kiganda Sub-county</rdfs:label>
    </owl:NamedIndividual>
    


    <!-- http://purl.obolibrary.org/obo/GAZ_00236496 -->

    <owl:NamedIndividual rdf:about="http://purl.obolibrary.org/obo/GAZ_00236496">
        <obo:RO_0001025 rdf:resource="http://purl.obolibrary.org/obo/GAZ_00015435"/>
        <obo:IAO_0000115>A fourth-level administrative division of Uganda.</obo:IAO_0000115>
        <oboInOwl:hasOBONamespace>GAZ</oboInOwl:hasOBONamespace>
        <oboInOwl:id>GAZ:00236496</oboInOwl:id>
        <rdfs:label>Myanzi Sub-county</rdfs:label>
    </owl:NamedIndividual>
    


    <!-- http://purl.obolibrary.org/obo/GAZ_00236497 -->

    <owl:NamedIndividual rdf:about="http://purl.obolibrary.org/obo/GAZ_00236497">
        <obo:RO_0001025 rdf:resource="http://purl.obolibrary.org/obo/GAZ_00015434"/>
        <obo:IAO_0000115>A fourth-level administrative division of Uganda.</obo:IAO_0000115>
        <oboInOwl:hasOBONamespace>GAZ</oboInOwl:hasOBONamespace>
        <oboInOwl:id>GAZ:00236497</oboInOwl:id>
        <rdfs:label>Bagezza Sub-county</rdfs:label>
    </owl:NamedIndividual>
    


    <!-- http://purl.obolibrary.org/obo/GAZ_00236498 -->

    <owl:NamedIndividual rdf:about="http://purl.obolibrary.org/obo/GAZ_00236498">
        <obo:RO_0001025 rdf:resource="http://purl.obolibrary.org/obo/GAZ_00015434"/>
        <obo:IAO_0000115>A fourth-level administrative division of Uganda.</obo:IAO_0000115>
        <oboInOwl:hasOBONamespace>GAZ</oboInOwl:hasOBONamespace>
        <oboInOwl:id>GAZ:00236498</oboInOwl:id>
        <rdfs:label>Butoloogo Sub-county</rdfs:label>
    </owl:NamedIndividual>
    


    <!-- http://purl.obolibrary.org/obo/GAZ_00236499 -->

    <owl:NamedIndividual rdf:about="http://purl.obolibrary.org/obo/GAZ_00236499">
        <obo:RO_0001025 rdf:resource="http://purl.obolibrary.org/obo/GAZ_00015434"/>
        <obo:IAO_0000115>A fourth-level administrative division of Uganda.</obo:IAO_0000115>
        <oboInOwl:hasOBONamespace>GAZ</oboInOwl:hasOBONamespace>
        <oboInOwl:id>GAZ:00236499</oboInOwl:id>
        <rdfs:label>Kasambya Sub-county</rdfs:label>
    </owl:NamedIndividual>
    


    <!-- http://purl.obolibrary.org/obo/GAZ_00236500 -->

    <owl:NamedIndividual rdf:about="http://purl.obolibrary.org/obo/GAZ_00236500">
        <obo:RO_0001025 rdf:resource="http://purl.obolibrary.org/obo/GAZ_00015434"/>
        <obo:IAO_0000115>A fourth-level administrative division of Uganda.</obo:IAO_0000115>
        <oboInOwl:hasOBONamespace>GAZ</oboInOwl:hasOBONamespace>
        <oboInOwl:id>GAZ:00236500</oboInOwl:id>
        <rdfs:label>Kitenga Sub-county</rdfs:label>
    </owl:NamedIndividual>
    


    <!-- http://purl.obolibrary.org/obo/GAZ_00236501 -->

    <owl:NamedIndividual rdf:about="http://purl.obolibrary.org/obo/GAZ_00236501">
        <obo:RO_0001025 rdf:resource="http://purl.obolibrary.org/obo/GAZ_00015434"/>
        <obo:IAO_0000115>A fourth-level administrative division of Uganda.</obo:IAO_0000115>
        <oboInOwl:hasOBONamespace>GAZ</oboInOwl:hasOBONamespace>
        <oboInOwl:id>GAZ:00236501</oboInOwl:id>
        <rdfs:label>Kiyuni Sub-county</rdfs:label>
    </owl:NamedIndividual>
    


    <!-- http://purl.obolibrary.org/obo/GAZ_00236502 -->

    <owl:NamedIndividual rdf:about="http://purl.obolibrary.org/obo/GAZ_00236502">
        <obo:RO_0001025 rdf:resource="http://purl.obolibrary.org/obo/GAZ_00015434"/>
        <obo:IAO_0000115>A fourth-level administrative division of Uganda.</obo:IAO_0000115>
        <oboInOwl:hasOBONamespace>GAZ</oboInOwl:hasOBONamespace>
        <oboInOwl:id>GAZ:00236502</oboInOwl:id>
        <rdfs:label>Madudu Sub-county</rdfs:label>
    </owl:NamedIndividual>
    


    <!-- http://purl.obolibrary.org/obo/GAZ_00236503 -->

    <owl:NamedIndividual rdf:about="http://purl.obolibrary.org/obo/GAZ_00236503">
        <obo:RO_0001025 rdf:resource="http://purl.obolibrary.org/obo/GAZ_00015434"/>
        <obo:IAO_0000115>A fourth-level administrative division of Uganda.</obo:IAO_0000115>
        <oboInOwl:hasOBONamespace>GAZ</oboInOwl:hasOBONamespace>
        <oboInOwl:id>GAZ:00236503</oboInOwl:id>
        <rdfs:label>Mubende Town</rdfs:label>
    </owl:NamedIndividual>
    


    <!-- http://purl.obolibrary.org/obo/GAZ_00236504 -->

    <owl:NamedIndividual rdf:about="http://purl.obolibrary.org/obo/GAZ_00236504">
        <obo:RO_0001025 rdf:resource="http://purl.obolibrary.org/obo/GAZ_00015342"/>
        <obo:IAO_0000115>A protected area protecting a rain forest. Located between Kampala and Jinja. Established 1932.</obo:IAO_0000115>
        <oboInOwl:hasOBONamespace>GAZ</oboInOwl:hasOBONamespace>
        <oboInOwl:id>GAZ:00236504</oboInOwl:id>
        <rdfs:label>Mabira Forest Reserve</rdfs:label>
    </owl:NamedIndividual>
    


    <!-- http://purl.obolibrary.org/obo/GAZ_00236505 -->

    <owl:NamedIndividual rdf:about="http://purl.obolibrary.org/obo/GAZ_00236505">
        <obo:RO_0001025 rdf:resource="http://purl.obolibrary.org/obo/GAZ_00015430"/>
        <obo:IAO_0000115>A fourth-level administrative division of Uganda.</obo:IAO_0000115>
        <oboInOwl:hasOBONamespace>GAZ</oboInOwl:hasOBONamespace>
        <oboInOwl:id>GAZ:00236505</oboInOwl:id>
        <rdfs:label>Bugaya Sub-county</rdfs:label>
    </owl:NamedIndividual>
    


    <!-- http://purl.obolibrary.org/obo/GAZ_00236506 -->

    <owl:NamedIndividual rdf:about="http://purl.obolibrary.org/obo/GAZ_00236506">
        <obo:RO_0001025 rdf:resource="http://purl.obolibrary.org/obo/GAZ_00015430"/>
        <obo:IAO_0000115>A fourth-level administrative division of Uganda.</obo:IAO_0000115>
        <oboInOwl:hasOBONamespace>GAZ</oboInOwl:hasOBONamespace>
        <oboInOwl:id>GAZ:00236506</oboInOwl:id>
        <rdfs:label>Busamuzi Sub-county</rdfs:label>
    </owl:NamedIndividual>
    


    <!-- http://purl.obolibrary.org/obo/GAZ_00236507 -->

    <owl:NamedIndividual rdf:about="http://purl.obolibrary.org/obo/GAZ_00236507">
        <obo:RO_0001025 rdf:resource="http://purl.obolibrary.org/obo/GAZ_00015430"/>
        <obo:IAO_0000115>A fourth-level administrative division of Uganda.</obo:IAO_0000115>
        <oboInOwl:hasOBONamespace>GAZ</oboInOwl:hasOBONamespace>
        <oboInOwl:id>GAZ:00236507</oboInOwl:id>
        <rdfs:label>Bweema Sub-county</rdfs:label>
    </owl:NamedIndividual>
    


    <!-- http://purl.obolibrary.org/obo/GAZ_00236508 -->

    <owl:NamedIndividual rdf:about="http://purl.obolibrary.org/obo/GAZ_00236508">
        <obo:RO_0001025 rdf:resource="http://purl.obolibrary.org/obo/GAZ_00015430"/>
        <obo:IAO_0000115>A fourth-level administrative division of Uganda.</obo:IAO_0000115>
        <oboInOwl:hasOBONamespace>GAZ</oboInOwl:hasOBONamespace>
        <oboInOwl:id>GAZ:00236508</oboInOwl:id>
        <rdfs:label>Nairambi Sub-county</rdfs:label>
    </owl:NamedIndividual>
    


    <!-- http://purl.obolibrary.org/obo/GAZ_00236509 -->

    <owl:NamedIndividual rdf:about="http://purl.obolibrary.org/obo/GAZ_00236509">
        <obo:RO_0001025 rdf:resource="http://purl.obolibrary.org/obo/GAZ_00015433"/>
        <obo:IAO_0000115>A fourth-level administrative division of Uganda.</obo:IAO_0000115>
        <oboInOwl:hasOBONamespace>GAZ</oboInOwl:hasOBONamespace>
        <oboInOwl:id>GAZ:00236509</oboInOwl:id>
        <rdfs:label>Buikwe Sub-county</rdfs:label>
    </owl:NamedIndividual>
    


    <!-- http://purl.obolibrary.org/obo/GAZ_00236510 -->

    <owl:NamedIndividual rdf:about="http://purl.obolibrary.org/obo/GAZ_00236510">
        <obo:RO_0001025 rdf:resource="http://purl.obolibrary.org/obo/GAZ_00015433"/>
        <obo:IAO_0000115>A fourth-level administrative division of Uganda.</obo:IAO_0000115>
        <oboInOwl:hasOBONamespace>GAZ</oboInOwl:hasOBONamespace>
        <oboInOwl:id>GAZ:00236510</oboInOwl:id>
        <rdfs:label>Kawolo Sub-county</rdfs:label>
    </owl:NamedIndividual>
    


    <!-- http://purl.obolibrary.org/obo/GAZ_00236511 -->

    <owl:NamedIndividual rdf:about="http://purl.obolibrary.org/obo/GAZ_00236511">
        <obo:RO_0001025 rdf:resource="http://purl.obolibrary.org/obo/GAZ_00015433"/>
        <obo:IAO_0000115>A fourth-level administrative division of Uganda.</obo:IAO_0000115>
        <oboInOwl:hasOBONamespace>GAZ</oboInOwl:hasOBONamespace>
        <oboInOwl:id>GAZ:00236511</oboInOwl:id>
        <rdfs:label>Lugazi Town</rdfs:label>
    </owl:NamedIndividual>
    


    <!-- http://purl.obolibrary.org/obo/GAZ_00236512 -->

    <owl:NamedIndividual rdf:about="http://purl.obolibrary.org/obo/GAZ_00236512">
        <obo:RO_0001025 rdf:resource="http://purl.obolibrary.org/obo/GAZ_00015433"/>
        <obo:IAO_0000115>A fourth-level administrative division of Uganda.</obo:IAO_0000115>
        <oboInOwl:hasOBONamespace>GAZ</oboInOwl:hasOBONamespace>
        <oboInOwl:id>GAZ:00236512</oboInOwl:id>
        <rdfs:label>Najja Sub-county</rdfs:label>
    </owl:NamedIndividual>
    


    <!-- http://purl.obolibrary.org/obo/GAZ_00236513 -->

    <owl:NamedIndividual rdf:about="http://purl.obolibrary.org/obo/GAZ_00236513">
        <obo:RO_0001025 rdf:resource="http://purl.obolibrary.org/obo/GAZ_00015433"/>
        <obo:IAO_0000115>A fourth-level administrative division of Uganda.</obo:IAO_0000115>
        <oboInOwl:hasOBONamespace>GAZ</oboInOwl:hasOBONamespace>
        <oboInOwl:id>GAZ:00236513</oboInOwl:id>
        <rdfs:label>Najjembe Sub-county</rdfs:label>
    </owl:NamedIndividual>
    


    <!-- http://purl.obolibrary.org/obo/GAZ_00236514 -->

    <owl:NamedIndividual rdf:about="http://purl.obolibrary.org/obo/GAZ_00236514">
        <obo:RO_0001025 rdf:resource="http://purl.obolibrary.org/obo/GAZ_00015433"/>
        <obo:IAO_0000115>A fourth-level administrative division of Uganda.</obo:IAO_0000115>
        <oboInOwl:hasOBONamespace>GAZ</oboInOwl:hasOBONamespace>
        <oboInOwl:id>GAZ:00236514</oboInOwl:id>
        <rdfs:label>Ngogwe Sub-county</rdfs:label>
    </owl:NamedIndividual>
    


    <!-- http://purl.obolibrary.org/obo/GAZ_00236515 -->

    <owl:NamedIndividual rdf:about="http://purl.obolibrary.org/obo/GAZ_00236515">
        <obo:RO_0001025 rdf:resource="http://purl.obolibrary.org/obo/GAZ_00015433"/>
        <obo:IAO_0000115>A fourth-level administrative division of Uganda.</obo:IAO_0000115>
        <oboInOwl:hasOBONamespace>GAZ</oboInOwl:hasOBONamespace>
        <oboInOwl:id>GAZ:00236515</oboInOwl:id>
        <rdfs:label>Njeru Town</rdfs:label>
    </owl:NamedIndividual>
    


    <!-- http://purl.obolibrary.org/obo/GAZ_00236516 -->

    <owl:NamedIndividual rdf:about="http://purl.obolibrary.org/obo/GAZ_00236516">
        <obo:RO_0001025 rdf:resource="http://purl.obolibrary.org/obo/GAZ_00015433"/>
        <obo:IAO_0000115>A fourth-level administrative division of Uganda.</obo:IAO_0000115>
        <oboInOwl:hasOBONamespace>GAZ</oboInOwl:hasOBONamespace>
        <oboInOwl:id>GAZ:00236516</oboInOwl:id>
        <rdfs:label>Nkonkonjeru Town</rdfs:label>
    </owl:NamedIndividual>
    


    <!-- http://purl.obolibrary.org/obo/GAZ_00236517 -->

    <owl:NamedIndividual rdf:about="http://purl.obolibrary.org/obo/GAZ_00236517">
        <obo:RO_0001025 rdf:resource="http://purl.obolibrary.org/obo/GAZ_00015433"/>
        <obo:IAO_0000115>A fourth-level administrative division of Uganda.</obo:IAO_0000115>
        <oboInOwl:hasOBONamespace>GAZ</oboInOwl:hasOBONamespace>
        <oboInOwl:id>GAZ:00236517</oboInOwl:id>
        <rdfs:label>Nyenga Sub-county</rdfs:label>
    </owl:NamedIndividual>
    


    <!-- http://purl.obolibrary.org/obo/GAZ_00236518 -->

    <owl:NamedIndividual rdf:about="http://purl.obolibrary.org/obo/GAZ_00236518">
        <obo:RO_0001025 rdf:resource="http://purl.obolibrary.org/obo/GAZ_00015433"/>
        <obo:IAO_0000115>A fourth-level administrative division of Uganda.</obo:IAO_0000115>
        <oboInOwl:hasOBONamespace>GAZ</oboInOwl:hasOBONamespace>
        <oboInOwl:id>GAZ:00236518</oboInOwl:id>
        <rdfs:label>Ssi-Bukunja Sub-county</rdfs:label>
    </owl:NamedIndividual>
    


    <!-- http://purl.obolibrary.org/obo/GAZ_00236519 -->

    <owl:NamedIndividual rdf:about="http://purl.obolibrary.org/obo/GAZ_00236519">
        <obo:RO_0001025 rdf:resource="http://purl.obolibrary.org/obo/GAZ_00015433"/>
        <obo:IAO_0000115>A fourth-level administrative division of Uganda.</obo:IAO_0000115>
        <oboInOwl:hasOBONamespace>GAZ</oboInOwl:hasOBONamespace>
        <oboInOwl:id>GAZ:00236519</oboInOwl:id>
        <rdfs:label>Wakisi Sub-county</rdfs:label>
    </owl:NamedIndividual>
    


    <!-- http://purl.obolibrary.org/obo/GAZ_00236520 -->

    <owl:NamedIndividual rdf:about="http://purl.obolibrary.org/obo/GAZ_00236520">
        <obo:RO_0001025 rdf:resource="http://purl.obolibrary.org/obo/GAZ_00015431"/>
        <obo:IAO_0000115>A fourth-level administrative division of Uganda.</obo:IAO_0000115>
        <oboInOwl:hasOBONamespace>GAZ</oboInOwl:hasOBONamespace>
        <oboInOwl:id>GAZ:00236520</oboInOwl:id>
        <rdfs:label>Goma Sub-County</rdfs:label>
    </owl:NamedIndividual>
    


    <!-- http://purl.obolibrary.org/obo/GAZ_00236521 -->

    <owl:NamedIndividual rdf:about="http://purl.obolibrary.org/obo/GAZ_00236521">
        <obo:RO_0001025 rdf:resource="http://purl.obolibrary.org/obo/GAZ_00015431"/>
        <obo:IAO_0000115>A fourth-level administrative division of Uganda.</obo:IAO_0000115>
        <oboInOwl:hasOBONamespace>GAZ</oboInOwl:hasOBONamespace>
        <oboInOwl:id>GAZ:00236521</oboInOwl:id>
        <rdfs:label>Kkome Islands Sub-County</rdfs:label>
    </owl:NamedIndividual>
    


    <!-- http://purl.obolibrary.org/obo/GAZ_00236522 -->

    <owl:NamedIndividual rdf:about="http://purl.obolibrary.org/obo/GAZ_00236522">
        <obo:RO_0001025 rdf:resource="http://purl.obolibrary.org/obo/GAZ_00015431"/>
        <obo:IAO_0000115>A fourth-level administrative division of Uganda.</obo:IAO_0000115>
        <oboInOwl:hasOBONamespace>GAZ</oboInOwl:hasOBONamespace>
        <oboInOwl:id>GAZ:00236522</oboInOwl:id>
        <rdfs:label>Kyampisi Sub-County</rdfs:label>
    </owl:NamedIndividual>
    


    <!-- http://purl.obolibrary.org/obo/GAZ_00236523 -->

    <owl:NamedIndividual rdf:about="http://purl.obolibrary.org/obo/GAZ_00236523">
        <obo:RO_0001025 rdf:resource="http://purl.obolibrary.org/obo/GAZ_00015431"/>
        <obo:IAO_0000115>A fourth-level administrative division of Uganda.</obo:IAO_0000115>
        <oboInOwl:hasOBONamespace>GAZ</oboInOwl:hasOBONamespace>
        <oboInOwl:id>GAZ:00236523</oboInOwl:id>
        <rdfs:label>Mukono Town</rdfs:label>
    </owl:NamedIndividual>
    


    <!-- http://purl.obolibrary.org/obo/GAZ_00236524 -->

    <owl:NamedIndividual rdf:about="http://purl.obolibrary.org/obo/GAZ_00236524">
        <obo:RO_0001025 rdf:resource="http://purl.obolibrary.org/obo/GAZ_00015431"/>
        <obo:IAO_0000115>A fourth-level administrative division of Uganda.</obo:IAO_0000115>
        <oboInOwl:hasOBONamespace>GAZ</oboInOwl:hasOBONamespace>
        <oboInOwl:id>GAZ:00236524</oboInOwl:id>
        <rdfs:label>Nakisunga Sub-County</rdfs:label>
    </owl:NamedIndividual>
    


    <!-- http://purl.obolibrary.org/obo/GAZ_00236525 -->

    <owl:NamedIndividual rdf:about="http://purl.obolibrary.org/obo/GAZ_00236525">
        <obo:RO_0001025 rdf:resource="http://purl.obolibrary.org/obo/GAZ_00015431"/>
        <obo:IAO_0000115>A fourth-level administrative division of Uganda.</obo:IAO_0000115>
        <oboInOwl:hasOBONamespace>GAZ</oboInOwl:hasOBONamespace>
        <oboInOwl:id>GAZ:00236525</oboInOwl:id>
        <rdfs:label>Nama Sub-County</rdfs:label>
    </owl:NamedIndividual>
    


    <!-- http://purl.obolibrary.org/obo/GAZ_00236526 -->

    <owl:NamedIndividual rdf:about="http://purl.obolibrary.org/obo/GAZ_00236526">
        <obo:RO_0001025 rdf:resource="http://purl.obolibrary.org/obo/GAZ_00015431"/>
        <obo:IAO_0000115>A fourth-level administrative division of Uganda.</obo:IAO_0000115>
        <oboInOwl:hasOBONamespace>GAZ</oboInOwl:hasOBONamespace>
        <oboInOwl:id>GAZ:00236526</oboInOwl:id>
        <rdfs:label>Ntenjeru Sub-County</rdfs:label>
    </owl:NamedIndividual>
    


    <!-- http://purl.obolibrary.org/obo/GAZ_00236527 -->

    <owl:NamedIndividual rdf:about="http://purl.obolibrary.org/obo/GAZ_00236527">
        <obo:RO_0001025 rdf:resource="http://purl.obolibrary.org/obo/GAZ_00015432"/>
        <obo:IAO_0000115>A fourth-level administrative division of Uganda.</obo:IAO_0000115>
        <oboInOwl:hasOBONamespace>GAZ</oboInOwl:hasOBONamespace>
        <oboInOwl:id>GAZ:00236527</oboInOwl:id>
        <rdfs:label>Kasawo Sub-county</rdfs:label>
    </owl:NamedIndividual>
    


    <!-- http://purl.obolibrary.org/obo/GAZ_00236528 -->

    <owl:NamedIndividual rdf:about="http://purl.obolibrary.org/obo/GAZ_00236528">
        <obo:RO_0001025 rdf:resource="http://purl.obolibrary.org/obo/GAZ_00015432"/>
        <obo:IAO_0000115>A fourth-level administrative division of Uganda.</obo:IAO_0000115>
        <oboInOwl:hasOBONamespace>GAZ</oboInOwl:hasOBONamespace>
        <oboInOwl:id>GAZ:00236528</oboInOwl:id>
        <rdfs:label>Kimenyedde Sub-county</rdfs:label>
    </owl:NamedIndividual>
    


    <!-- http://purl.obolibrary.org/obo/GAZ_00236529 -->

    <owl:NamedIndividual rdf:about="http://purl.obolibrary.org/obo/GAZ_00236529">
        <obo:RO_0001025 rdf:resource="http://purl.obolibrary.org/obo/GAZ_00015432"/>
        <obo:IAO_0000115>A fourth-level administrative division of Uganda.</obo:IAO_0000115>
        <oboInOwl:hasOBONamespace>GAZ</oboInOwl:hasOBONamespace>
        <oboInOwl:id>GAZ:00236529</oboInOwl:id>
        <rdfs:label>Nabaale Sub-county</rdfs:label>
    </owl:NamedIndividual>
    


    <!-- http://purl.obolibrary.org/obo/GAZ_00236530 -->

    <owl:NamedIndividual rdf:about="http://purl.obolibrary.org/obo/GAZ_00236530">
        <obo:RO_0001025 rdf:resource="http://purl.obolibrary.org/obo/GAZ_00015432"/>
        <obo:IAO_0000115>A fourth-level administrative division of Uganda.</obo:IAO_0000115>
        <oboInOwl:hasOBONamespace>GAZ</oboInOwl:hasOBONamespace>
        <oboInOwl:id>GAZ:00236530</oboInOwl:id>
        <rdfs:label>Nagojje Sub-county</rdfs:label>
    </owl:NamedIndividual>
    


    <!-- http://purl.obolibrary.org/obo/GAZ_00236531 -->

    <owl:NamedIndividual rdf:about="http://purl.obolibrary.org/obo/GAZ_00236531">
        <obo:RO_0001025 rdf:resource="http://purl.obolibrary.org/obo/GAZ_00015432"/>
        <obo:IAO_0000115>A fourth-level administrative division of Uganda.</obo:IAO_0000115>
        <oboInOwl:hasOBONamespace>GAZ</oboInOwl:hasOBONamespace>
        <oboInOwl:id>GAZ:00236531</oboInOwl:id>
        <rdfs:label>Ntunda Sub-county</rdfs:label>
    </owl:NamedIndividual>
    


    <!-- http://purl.obolibrary.org/obo/GAZ_00236532 -->

    <owl:NamedIndividual rdf:about="http://purl.obolibrary.org/obo/GAZ_00236532">
        <obo:RO_0001025 rdf:resource="http://purl.obolibrary.org/obo/GAZ_00015432"/>
        <obo:IAO_0000115>A fourth-level administrative division of Uganda.</obo:IAO_0000115>
        <oboInOwl:hasOBONamespace>GAZ</oboInOwl:hasOBONamespace>
        <oboInOwl:id>GAZ:00236532</oboInOwl:id>
        <rdfs:label>Seeta-Namuganga Sub-county</rdfs:label>
    </owl:NamedIndividual>
    


    <!-- http://purl.obolibrary.org/obo/GAZ_00236533 -->

    <owl:NamedIndividual rdf:about="http://purl.obolibrary.org/obo/GAZ_00236533">
        <obo:RO_0001025 rdf:resource="http://purl.obolibrary.org/obo/GAZ_00236523"/>
        <obo:IAO_0000115>An administrative ward (township) of Mukuno Town.</obo:IAO_0000115>
        <oboInOwl:hasOBONamespace>GAZ</oboInOwl:hasOBONamespace>
        <oboInOwl:id>GAZ:00236533</oboInOwl:id>
        <rdfs:label>Ggulu Ward</rdfs:label>
    </owl:NamedIndividual>
    


    <!-- http://purl.obolibrary.org/obo/GAZ_00236534 -->

    <owl:NamedIndividual rdf:about="http://purl.obolibrary.org/obo/GAZ_00236534">
        <obo:RO_0001025 rdf:resource="http://purl.obolibrary.org/obo/GAZ_00236523"/>
        <obo:IAO_0000115>An administrative ward (township) of Mukuno Town.</obo:IAO_0000115>
        <oboInOwl:hasOBONamespace>GAZ</oboInOwl:hasOBONamespace>
        <oboInOwl:id>GAZ:00236534</oboInOwl:id>
        <rdfs:label>Nsuube Ward</rdfs:label>
    </owl:NamedIndividual>
    


    <!-- http://purl.obolibrary.org/obo/GAZ_00236535 -->

    <owl:NamedIndividual rdf:about="http://purl.obolibrary.org/obo/GAZ_00236535">
        <obo:RO_0001025 rdf:resource="http://purl.obolibrary.org/obo/GAZ_00236523"/>
        <obo:IAO_0000115>An administrative ward (township) of Mukuno Town.</obo:IAO_0000115>
        <oboInOwl:hasOBONamespace>GAZ</oboInOwl:hasOBONamespace>
        <oboInOwl:id>GAZ:00236535</oboInOwl:id>
        <rdfs:label>Namumira Ward</rdfs:label>
    </owl:NamedIndividual>
    


    <!-- http://purl.obolibrary.org/obo/GAZ_00236536 -->

    <owl:NamedIndividual rdf:about="http://purl.obolibrary.org/obo/GAZ_00236536">
        <obo:RO_0001025 rdf:resource="http://purl.obolibrary.org/obo/GAZ_00236523"/>
        <obo:IAO_0000115>An administrative ward (township) of Mukuno Town.</obo:IAO_0000115>
        <oboInOwl:hasOBONamespace>GAZ</oboInOwl:hasOBONamespace>
        <oboInOwl:id>GAZ:00236536</oboInOwl:id>
        <rdfs:label>Ntaawo Ward</rdfs:label>
    </owl:NamedIndividual>
    


    <!-- http://purl.obolibrary.org/obo/GAZ_00236537 -->

    <owl:NamedIndividual rdf:about="http://purl.obolibrary.org/obo/GAZ_00236537">
        <obo:RO_0001025 rdf:resource="http://purl.obolibrary.org/obo/GAZ_00236546"/>
        <obo:IAO_0000115>A fourth-level administrative division of Uganda.</obo:IAO_0000115>
        <oboInOwl:hasOBONamespace>GAZ</oboInOwl:hasOBONamespace>
        <oboInOwl:id>GAZ:00236537</oboInOwl:id>
        <rdfs:label>Kakooge Sub-County</rdfs:label>
    </owl:NamedIndividual>
    


    <!-- http://purl.obolibrary.org/obo/GAZ_00236538 -->

    <owl:NamedIndividual rdf:about="http://purl.obolibrary.org/obo/GAZ_00236538">
        <obo:RO_0001025 rdf:resource="http://purl.obolibrary.org/obo/GAZ_00236546"/>
        <obo:IAO_0000115>A fourth-level administrative division of Uganda.</obo:IAO_0000115>
        <oboInOwl:hasOBONamespace>GAZ</oboInOwl:hasOBONamespace>
        <oboInOwl:id>GAZ:00236538</oboInOwl:id>
        <rdfs:label>Kalongo Sub-County</rdfs:label>
    </owl:NamedIndividual>
    


    <!-- http://purl.obolibrary.org/obo/GAZ_00236539 -->

    <owl:NamedIndividual rdf:about="http://purl.obolibrary.org/obo/GAZ_00236539">
        <obo:RO_0001025 rdf:resource="http://purl.obolibrary.org/obo/GAZ_00236546"/>
        <obo:IAO_0000115>A fourth-level administrative division of Uganda.</obo:IAO_0000115>
        <oboInOwl:hasOBONamespace>GAZ</oboInOwl:hasOBONamespace>
        <oboInOwl:id>GAZ:00236539</oboInOwl:id>
        <rdfs:label>Kalungi Sub-County</rdfs:label>
    </owl:NamedIndividual>
    


    <!-- http://purl.obolibrary.org/obo/GAZ_00236540 -->

    <owl:NamedIndividual rdf:about="http://purl.obolibrary.org/obo/GAZ_00236540">
        <obo:RO_0001025 rdf:resource="http://purl.obolibrary.org/obo/GAZ_00236547"/>
        <obo:IAO_0000115>A fourth-level administrative division of Uganda.</obo:IAO_0000115>
        <oboInOwl:hasOBONamespace>GAZ</oboInOwl:hasOBONamespace>
        <oboInOwl:id>GAZ:00236540</oboInOwl:id>
        <rdfs:label>Lwabyata Sub-County</rdfs:label>
    </owl:NamedIndividual>
    


    <!-- http://purl.obolibrary.org/obo/GAZ_00236541 -->

    <owl:NamedIndividual rdf:about="http://purl.obolibrary.org/obo/GAZ_00236541">
        <obo:RO_0001025 rdf:resource="http://purl.obolibrary.org/obo/GAZ_00015428"/>
        <obo:IAO_0000115>A fourth-level administrative division of Uganda.</obo:IAO_0000115>
        <oboInOwl:hasOBONamespace>GAZ</oboInOwl:hasOBONamespace>
        <oboInOwl:id>GAZ:00236541</oboInOwl:id>
        <rdfs:label>Lwampanga Sub-County</rdfs:label>
    </owl:NamedIndividual>
    


    <!-- http://purl.obolibrary.org/obo/GAZ_00236542 -->

    <owl:NamedIndividual rdf:about="http://purl.obolibrary.org/obo/GAZ_00236542">
        <obo:RO_0001025 rdf:resource="http://purl.obolibrary.org/obo/GAZ_00236547"/>
        <obo:IAO_0000115>A fourth-level administrative division of Uganda.</obo:IAO_0000115>
        <oboInOwl:hasOBONamespace>GAZ</oboInOwl:hasOBONamespace>
        <oboInOwl:id>GAZ:00236542</oboInOwl:id>
        <rdfs:label>Nabiswera Sub-County</rdfs:label>
    </owl:NamedIndividual>
    


    <!-- http://purl.obolibrary.org/obo/GAZ_00236543 -->

    <owl:NamedIndividual rdf:about="http://purl.obolibrary.org/obo/GAZ_00236543">
        <obo:RO_0001025 rdf:resource="http://purl.obolibrary.org/obo/GAZ_00015428"/>
        <obo:IAO_0000115>A fourth-level administrative division of Uganda.</obo:IAO_0000115>
        <oboInOwl:hasOBONamespace>GAZ</oboInOwl:hasOBONamespace>
        <oboInOwl:id>GAZ:00236543</oboInOwl:id>
        <rdfs:label>Nakasongola Town</rdfs:label>
    </owl:NamedIndividual>
    


    <!-- http://purl.obolibrary.org/obo/GAZ_00236544 -->

    <owl:NamedIndividual rdf:about="http://purl.obolibrary.org/obo/GAZ_00236544">
        <obo:RO_0001025 rdf:resource="http://purl.obolibrary.org/obo/GAZ_00236547"/>
        <obo:IAO_0000115>A fourth-level administrative division of Uganda.</obo:IAO_0000115>
        <oboInOwl:hasOBONamespace>GAZ</oboInOwl:hasOBONamespace>
        <oboInOwl:id>GAZ:00236544</oboInOwl:id>
        <rdfs:label>Nakitoma Sub-County</rdfs:label>
    </owl:NamedIndividual>
    


    <!-- http://purl.obolibrary.org/obo/GAZ_00236545 -->

    <owl:NamedIndividual rdf:about="http://purl.obolibrary.org/obo/GAZ_00236545">
        <obo:RO_0001025 rdf:resource="http://purl.obolibrary.org/obo/GAZ_00015428"/>
        <obo:IAO_0000115>A fourth-level administrative division of Uganda.</obo:IAO_0000115>
        <oboInOwl:hasOBONamespace>GAZ</oboInOwl:hasOBONamespace>
        <oboInOwl:id>GAZ:00236545</oboInOwl:id>
        <rdfs:label>Wabinyonyi Sub-County</rdfs:label>
    </owl:NamedIndividual>
    


    <!-- http://purl.obolibrary.org/obo/GAZ_00236546 -->

    <owl:NamedIndividual rdf:about="http://purl.obolibrary.org/obo/GAZ_00236546">
        <obo:RO_0001025 rdf:resource="http://purl.obolibrary.org/obo/GAZ_00015348"/>
        <obo:IAO_0000115>A third-level administrative division of Uganda.</obo:IAO_0000115>
        <oboInOwl:hasOBONamespace>GAZ</oboInOwl:hasOBONamespace>
        <oboInOwl:id>GAZ:00236546</oboInOwl:id>
        <rdfs:label>Kyabujingo County</rdfs:label>
    </owl:NamedIndividual>
    


    <!-- http://purl.obolibrary.org/obo/GAZ_00236547 -->

    <owl:NamedIndividual rdf:about="http://purl.obolibrary.org/obo/GAZ_00236547">
        <obo:RO_0001025 rdf:resource="http://purl.obolibrary.org/obo/GAZ_00015348"/>
        <obo:IAO_0000115>A third-level administrative division of Uganda.</obo:IAO_0000115>
        <oboInOwl:hasOBONamespace>GAZ</oboInOwl:hasOBONamespace>
        <oboInOwl:id>GAZ:00236547</oboInOwl:id>
        <rdfs:label>Budyebo County</rdfs:label>
    </owl:NamedIndividual>
    


    <!-- http://purl.obolibrary.org/obo/GAZ_00236548 -->

    <owl:NamedIndividual rdf:about="http://purl.obolibrary.org/obo/GAZ_00236548">
        <obo:RO_0001025 rdf:resource="http://purl.obolibrary.org/obo/GAZ_00015427"/>
        <obo:IAO_0000115>A fourth-level administrative division of Uganda.</obo:IAO_0000115>
        <oboInOwl:hasOBONamespace>GAZ</oboInOwl:hasOBONamespace>
        <oboInOwl:id>GAZ:00236548</oboInOwl:id>
        <rdfs:label>Kaliiro Sub-county</rdfs:label>
    </owl:NamedIndividual>
    


    <!-- http://purl.obolibrary.org/obo/GAZ_00236549 -->

    <owl:NamedIndividual rdf:about="http://purl.obolibrary.org/obo/GAZ_00236549">
        <obo:RO_0001025 rdf:resource="http://purl.obolibrary.org/obo/GAZ_00015427"/>
        <obo:IAO_0000115>A fourth-level administrative division of Uganda.</obo:IAO_0000115>
        <oboInOwl:hasOBONamespace>GAZ</oboInOwl:hasOBONamespace>
        <oboInOwl:id>GAZ:00236549</oboInOwl:id>
        <rdfs:label>Kasagama Sub-county</rdfs:label>
    </owl:NamedIndividual>
    


    <!-- http://purl.obolibrary.org/obo/GAZ_00236550 -->

    <owl:NamedIndividual rdf:about="http://purl.obolibrary.org/obo/GAZ_00236550">
        <obo:RO_0001025 rdf:resource="http://purl.obolibrary.org/obo/GAZ_00015427"/>
        <obo:IAO_0000115>A fourth-level administrative division of Uganda.</obo:IAO_0000115>
        <oboInOwl:hasOBONamespace>GAZ</oboInOwl:hasOBONamespace>
        <oboInOwl:id>GAZ:00236550</oboInOwl:id>
        <rdfs:label>Kinuuka Sub-county</rdfs:label>
    </owl:NamedIndividual>
    


    <!-- http://purl.obolibrary.org/obo/GAZ_00236551 -->

    <owl:NamedIndividual rdf:about="http://purl.obolibrary.org/obo/GAZ_00236551">
        <obo:RO_0001025 rdf:resource="http://purl.obolibrary.org/obo/GAZ_00015427"/>
        <obo:IAO_0000115>A fourth-level administrative division of Uganda.</obo:IAO_0000115>
        <oboInOwl:hasOBONamespace>GAZ</oboInOwl:hasOBONamespace>
        <oboInOwl:id>GAZ:00236551</oboInOwl:id>
        <rdfs:label>Lyantonde Town</rdfs:label>
    </owl:NamedIndividual>
    


    <!-- http://purl.obolibrary.org/obo/GAZ_00236552 -->

    <owl:NamedIndividual rdf:about="http://purl.obolibrary.org/obo/GAZ_00236552">
        <obo:RO_0001025 rdf:resource="http://purl.obolibrary.org/obo/GAZ_00015427"/>
        <obo:IAO_0000115>A fourth-level administrative division of Uganda.</obo:IAO_0000115>
        <oboInOwl:hasOBONamespace>GAZ</oboInOwl:hasOBONamespace>
        <oboInOwl:id>GAZ:00236552</oboInOwl:id>
        <rdfs:label>Mpumudde Sub-county</rdfs:label>
    </owl:NamedIndividual>
    


    <!-- http://purl.obolibrary.org/obo/GAZ_00236553 -->

    <owl:NamedIndividual rdf:about="http://purl.obolibrary.org/obo/GAZ_00236553">
        <obo:RO_0001025 rdf:resource="http://purl.obolibrary.org/obo/GAZ_00015424"/>
        <obo:IAO_0000115>A fourth-level administrative division of Uganda.</obo:IAO_0000115>
        <oboInOwl:hasOBONamespace>GAZ</oboInOwl:hasOBONamespace>
        <oboInOwl:id>GAZ:00236553</oboInOwl:id>
        <rdfs:label>Kakuuto Sub-county</rdfs:label>
    </owl:NamedIndividual>
    


    <!-- http://purl.obolibrary.org/obo/GAZ_00236554 -->

    <owl:NamedIndividual rdf:about="http://purl.obolibrary.org/obo/GAZ_00236554">
        <obo:RO_0001025 rdf:resource="http://purl.obolibrary.org/obo/GAZ_00015424"/>
        <obo:IAO_0000115>A fourth-level administrative division of Uganda.</obo:IAO_0000115>
        <oboInOwl:hasOBONamespace>GAZ</oboInOwl:hasOBONamespace>
        <oboInOwl:id>GAZ:00236554</oboInOwl:id>
        <rdfs:label>Kasasa Sub-county</rdfs:label>
    </owl:NamedIndividual>
    


    <!-- http://purl.obolibrary.org/obo/GAZ_00236555 -->

    <owl:NamedIndividual rdf:about="http://purl.obolibrary.org/obo/GAZ_00236555">
        <obo:RO_0001025 rdf:resource="http://purl.obolibrary.org/obo/GAZ_00015424"/>
        <obo:IAO_0000115>A fourth-level administrative division of Uganda.</obo:IAO_0000115>
        <oboInOwl:hasOBONamespace>GAZ</oboInOwl:hasOBONamespace>
        <oboInOwl:id>GAZ:00236555</oboInOwl:id>
        <rdfs:label>Kibanda Sub-county</rdfs:label>
    </owl:NamedIndividual>
    


    <!-- http://purl.obolibrary.org/obo/GAZ_00236556 -->

    <owl:NamedIndividual rdf:about="http://purl.obolibrary.org/obo/GAZ_00236556">
        <obo:RO_0001025 rdf:resource="http://purl.obolibrary.org/obo/GAZ_00015424"/>
        <obo:IAO_0000115>A fourth-level administrative division of Uganda.</obo:IAO_0000115>
        <oboInOwl:hasOBONamespace>GAZ</oboInOwl:hasOBONamespace>
        <oboInOwl:id>GAZ:00236556</oboInOwl:id>
        <rdfs:label>Kifamba Sub-county</rdfs:label>
    </owl:NamedIndividual>
    


    <!-- http://purl.obolibrary.org/obo/GAZ_00236557 -->

    <owl:NamedIndividual rdf:about="http://purl.obolibrary.org/obo/GAZ_00236557">
        <obo:RO_0001025 rdf:resource="http://purl.obolibrary.org/obo/GAZ_00015424"/>
        <obo:IAO_0000115>A fourth-level administrative division of Uganda.</obo:IAO_0000115>
        <oboInOwl:hasOBONamespace>GAZ</oboInOwl:hasOBONamespace>
        <oboInOwl:id>GAZ:00236557</oboInOwl:id>
        <rdfs:label>Kyebe Sub-county</rdfs:label>
    </owl:NamedIndividual>
    


    <!-- http://purl.obolibrary.org/obo/GAZ_00236558 -->

    <owl:NamedIndividual rdf:about="http://purl.obolibrary.org/obo/GAZ_00236558">
        <obo:RO_0001025 rdf:resource="http://purl.obolibrary.org/obo/GAZ_00015425"/>
        <obo:IAO_0000115>A fourth-level administrative division of Uganda.</obo:IAO_0000115>
        <oboInOwl:hasOBONamespace>GAZ</oboInOwl:hasOBONamespace>
        <oboInOwl:id>GAZ:00236558</oboInOwl:id>
        <rdfs:label>Byakabanda Sub-county</rdfs:label>
    </owl:NamedIndividual>
    


    <!-- http://purl.obolibrary.org/obo/GAZ_00236559 -->

    <owl:NamedIndividual rdf:about="http://purl.obolibrary.org/obo/GAZ_00236559">
        <obo:RO_0001025 rdf:resource="http://purl.obolibrary.org/obo/GAZ_00015425"/>
        <obo:IAO_0000115>A fourth-level administrative division of Uganda.</obo:IAO_0000115>
        <oboInOwl:hasOBONamespace>GAZ</oboInOwl:hasOBONamespace>
        <oboInOwl:id>GAZ:00236559</oboInOwl:id>
        <rdfs:label>Ddwaniro Sub-county</rdfs:label>
    </owl:NamedIndividual>
    


    <!-- http://purl.obolibrary.org/obo/GAZ_00236560 -->

    <owl:NamedIndividual rdf:about="http://purl.obolibrary.org/obo/GAZ_00236560">
        <obo:RO_0001025 rdf:resource="http://purl.obolibrary.org/obo/GAZ_00015425"/>
        <obo:IAO_0000115>A fourth-level administrative division of Uganda.</obo:IAO_0000115>
        <oboInOwl:hasOBONamespace>GAZ</oboInOwl:hasOBONamespace>
        <oboInOwl:id>GAZ:00236560</oboInOwl:id>
        <rdfs:label>Kacheera Sub-county</rdfs:label>
    </owl:NamedIndividual>
    


    <!-- http://purl.obolibrary.org/obo/GAZ_00236561 -->

    <owl:NamedIndividual rdf:about="http://purl.obolibrary.org/obo/GAZ_00236561">
        <obo:RO_0001025 rdf:resource="http://purl.obolibrary.org/obo/GAZ_00015425"/>
        <obo:IAO_0000115>A fourth-level administrative division of Uganda.</obo:IAO_0000115>
        <oboInOwl:hasOBONamespace>GAZ</oboInOwl:hasOBONamespace>
        <oboInOwl:id>GAZ:00236561</oboInOwl:id>
        <rdfs:label>Kagamba Sub-county</rdfs:label>
    </owl:NamedIndividual>
    


    <!-- http://purl.obolibrary.org/obo/GAZ_00236562 -->

    <owl:NamedIndividual rdf:about="http://purl.obolibrary.org/obo/GAZ_00236562">
        <obo:RO_0001025 rdf:resource="http://purl.obolibrary.org/obo/GAZ_00015425"/>
        <obo:IAO_0000115>A fourth-level administrative division of Uganda.</obo:IAO_0000115>
        <oboInOwl:hasOBONamespace>GAZ</oboInOwl:hasOBONamespace>
        <oboInOwl:id>GAZ:00236562</oboInOwl:id>
        <rdfs:label>Kyalulangira Sub-county</rdfs:label>
    </owl:NamedIndividual>
    


    <!-- http://purl.obolibrary.org/obo/GAZ_00236563 -->

    <owl:NamedIndividual rdf:about="http://purl.obolibrary.org/obo/GAZ_00236563">
        <obo:RO_0001025 rdf:resource="http://purl.obolibrary.org/obo/GAZ_00015425"/>
        <obo:IAO_0000115>A fourth-level administrative division of Uganda.</obo:IAO_0000115>
        <oboInOwl:hasOBONamespace>GAZ</oboInOwl:hasOBONamespace>
        <oboInOwl:id>GAZ:00236563</oboInOwl:id>
        <rdfs:label>Lwamaggwa Sub-county</rdfs:label>
    </owl:NamedIndividual>
    


    <!-- http://purl.obolibrary.org/obo/GAZ_00236564 -->

    <owl:NamedIndividual rdf:about="http://purl.obolibrary.org/obo/GAZ_00236564">
        <obo:RO_0001025 rdf:resource="http://purl.obolibrary.org/obo/GAZ_00015425"/>
        <obo:IAO_0000115>A fourth-level administrative division of Uganda.</obo:IAO_0000115>
        <oboInOwl:hasOBONamespace>GAZ</oboInOwl:hasOBONamespace>
        <oboInOwl:id>GAZ:00236564</oboInOwl:id>
        <rdfs:label>Lwanda Sub-county</rdfs:label>
    </owl:NamedIndividual>
    


    <!-- http://purl.obolibrary.org/obo/GAZ_00236565 -->

    <owl:NamedIndividual rdf:about="http://purl.obolibrary.org/obo/GAZ_00236565">
        <obo:RO_0001025 rdf:resource="http://purl.obolibrary.org/obo/GAZ_00015425"/>
        <obo:IAO_0000115>A fourth-level administrative division of Uganda.</obo:IAO_0000115>
        <oboInOwl:hasOBONamespace>GAZ</oboInOwl:hasOBONamespace>
        <oboInOwl:id>GAZ:00236565</oboInOwl:id>
        <rdfs:label>Rakai Town</rdfs:label>
    </owl:NamedIndividual>
    


    <!-- http://purl.obolibrary.org/obo/GAZ_00236566 -->

    <owl:NamedIndividual rdf:about="http://purl.obolibrary.org/obo/GAZ_00236566">
        <obo:RO_0001025 rdf:resource="http://purl.obolibrary.org/obo/GAZ_00015426"/>
        <obo:IAO_0000115>A fourth-level administrative division of Uganda.</obo:IAO_0000115>
        <oboInOwl:hasOBONamespace>GAZ</oboInOwl:hasOBONamespace>
        <oboInOwl:id>GAZ:00236566</oboInOwl:id>
        <rdfs:label>Kabira Sub-county</rdfs:label>
    </owl:NamedIndividual>
    


    <!-- http://purl.obolibrary.org/obo/GAZ_00236567 -->

    <owl:NamedIndividual rdf:about="http://purl.obolibrary.org/obo/GAZ_00236567">
        <obo:RO_0001025 rdf:resource="http://purl.obolibrary.org/obo/GAZ_00015426"/>
        <obo:IAO_0000115>A fourth-level administrative division of Uganda.</obo:IAO_0000115>
        <oboInOwl:hasOBONamespace>GAZ</oboInOwl:hasOBONamespace>
        <oboInOwl:id>GAZ:00236567</oboInOwl:id>
        <rdfs:label>Kalisizo Sub-county</rdfs:label>
    </owl:NamedIndividual>
    


    <!-- http://purl.obolibrary.org/obo/GAZ_00236568 -->

    <owl:NamedIndividual rdf:about="http://purl.obolibrary.org/obo/GAZ_00236568">
        <obo:RO_0001025 rdf:resource="http://purl.obolibrary.org/obo/GAZ_00015426"/>
        <obo:IAO_0000115>A fourth-level administrative division of Uganda.</obo:IAO_0000115>
        <oboInOwl:hasOBONamespace>GAZ</oboInOwl:hasOBONamespace>
        <oboInOwl:id>GAZ:00236568</oboInOwl:id>
        <rdfs:label>Kasaali Sub-county</rdfs:label>
    </owl:NamedIndividual>
    


    <!-- http://purl.obolibrary.org/obo/GAZ_00236569 -->

    <owl:NamedIndividual rdf:about="http://purl.obolibrary.org/obo/GAZ_00236569">
        <obo:RO_0001025 rdf:resource="http://purl.obolibrary.org/obo/GAZ_00015426"/>
        <obo:IAO_0000115>A fourth-level administrative division of Uganda.</obo:IAO_0000115>
        <oboInOwl:hasOBONamespace>GAZ</oboInOwl:hasOBONamespace>
        <oboInOwl:id>GAZ:00236569</oboInOwl:id>
        <rdfs:label>Kirumba Sub-county</rdfs:label>
    </owl:NamedIndividual>
    


    <!-- http://purl.obolibrary.org/obo/GAZ_00236570 -->

    <owl:NamedIndividual rdf:about="http://purl.obolibrary.org/obo/GAZ_00236570">
        <obo:RO_0001025 rdf:resource="http://purl.obolibrary.org/obo/GAZ_00015426"/>
        <obo:IAO_0000115>A fourth-level administrative division of Uganda.</obo:IAO_0000115>
        <oboInOwl:hasOBONamespace>GAZ</oboInOwl:hasOBONamespace>
        <oboInOwl:id>GAZ:00236570</oboInOwl:id>
        <rdfs:label>Kyotera Town</rdfs:label>
    </owl:NamedIndividual>
    


    <!-- http://purl.obolibrary.org/obo/GAZ_00236571 -->

    <owl:NamedIndividual rdf:about="http://purl.obolibrary.org/obo/GAZ_00236571">
        <obo:RO_0001025 rdf:resource="http://purl.obolibrary.org/obo/GAZ_00015426"/>
        <obo:IAO_0000115>A fourth-level administrative division of Uganda.</obo:IAO_0000115>
        <oboInOwl:hasOBONamespace>GAZ</oboInOwl:hasOBONamespace>
        <oboInOwl:id>GAZ:00236571</oboInOwl:id>
        <rdfs:label>Lwankoni Sub-county</rdfs:label>
    </owl:NamedIndividual>
    


    <!-- http://purl.obolibrary.org/obo/GAZ_00236572 -->

    <owl:NamedIndividual rdf:about="http://purl.obolibrary.org/obo/GAZ_00236572">
        <obo:RO_0001025 rdf:resource="http://purl.obolibrary.org/obo/GAZ_00015426"/>
        <obo:IAO_0000115>A fourth-level administrative division of Uganda.</obo:IAO_0000115>
        <oboInOwl:hasOBONamespace>GAZ</oboInOwl:hasOBONamespace>
        <oboInOwl:id>GAZ:00236572</oboInOwl:id>
        <rdfs:label>Nabigasa Sub-county</rdfs:label>
    </owl:NamedIndividual>
    


    <!-- http://purl.obolibrary.org/obo/GAZ_00236573 -->

    <owl:NamedIndividual rdf:about="http://purl.obolibrary.org/obo/GAZ_00236573">
        <obo:RO_0001025 rdf:resource="http://purl.obolibrary.org/obo/GAZ_00015422"/>
        <obo:IAO_0000115>A fourth-level administrative division of Uganda.</obo:IAO_0000115>
        <oboInOwl:hasOBONamespace>GAZ</oboInOwl:hasOBONamespace>
        <oboInOwl:id>GAZ:00236573</oboInOwl:id>
        <rdfs:label>Lwemiyaga Sub-county</rdfs:label>
    </owl:NamedIndividual>
    


    <!-- http://purl.obolibrary.org/obo/GAZ_00236574 -->

    <owl:NamedIndividual rdf:about="http://purl.obolibrary.org/obo/GAZ_00236574">
        <obo:RO_0001025 rdf:resource="http://purl.obolibrary.org/obo/GAZ_00015422"/>
        <obo:IAO_0000115>A fourth-level administrative division of Uganda.</obo:IAO_0000115>
        <oboInOwl:hasOBONamespace>GAZ</oboInOwl:hasOBONamespace>
        <oboInOwl:id>GAZ:00236574</oboInOwl:id>
        <rdfs:label>Ntusi Sub-county</rdfs:label>
    </owl:NamedIndividual>
    


    <!-- http://purl.obolibrary.org/obo/GAZ_00236575 -->

    <owl:NamedIndividual rdf:about="http://purl.obolibrary.org/obo/GAZ_00236575">
        <obo:RO_0001025 rdf:resource="http://purl.obolibrary.org/obo/GAZ_00015423"/>
        <obo:IAO_0000115>A fourth-level administrative division of Uganda.</obo:IAO_0000115>
        <oboInOwl:hasOBONamespace>GAZ</oboInOwl:hasOBONamespace>
        <oboInOwl:id>GAZ:00236575</oboInOwl:id>
        <rdfs:label>Lugusulu Sub-county</rdfs:label>
    </owl:NamedIndividual>
    


    <!-- http://purl.obolibrary.org/obo/GAZ_00236576 -->

    <owl:NamedIndividual rdf:about="http://purl.obolibrary.org/obo/GAZ_00236576">
        <obo:RO_0001025 rdf:resource="http://purl.obolibrary.org/obo/GAZ_00015423"/>
        <obo:IAO_0000115>A fourth-level administrative division of Uganda.</obo:IAO_0000115>
        <oboInOwl:hasOBONamespace>GAZ</oboInOwl:hasOBONamespace>
        <oboInOwl:id>GAZ:00236576</oboInOwl:id>
        <rdfs:label>Lwebitakuli Sub-county</rdfs:label>
    </owl:NamedIndividual>
    


    <!-- http://purl.obolibrary.org/obo/GAZ_00236577 -->

    <owl:NamedIndividual rdf:about="http://purl.obolibrary.org/obo/GAZ_00236577">
        <obo:RO_0001025 rdf:resource="http://purl.obolibrary.org/obo/GAZ_00015423"/>
        <obo:IAO_0000115>A fourth-level administrative division of Uganda.</obo:IAO_0000115>
        <oboInOwl:hasOBONamespace>GAZ</oboInOwl:hasOBONamespace>
        <oboInOwl:id>GAZ:00236577</oboInOwl:id>
        <rdfs:label>Mateete Sub-county</rdfs:label>
    </owl:NamedIndividual>
    


    <!-- http://purl.obolibrary.org/obo/GAZ_00236578 -->

    <owl:NamedIndividual rdf:about="http://purl.obolibrary.org/obo/GAZ_00236578">
        <obo:RO_0001025 rdf:resource="http://purl.obolibrary.org/obo/GAZ_00015423"/>
        <obo:IAO_0000115>A fourth-level administrative division of Uganda.</obo:IAO_0000115>
        <oboInOwl:hasOBONamespace>GAZ</oboInOwl:hasOBONamespace>
        <oboInOwl:id>GAZ:00236578</oboInOwl:id>
        <rdfs:label>Mijwala Sub-county</rdfs:label>
    </owl:NamedIndividual>
    


    <!-- http://purl.obolibrary.org/obo/GAZ_00236579 -->

    <owl:NamedIndividual rdf:about="http://purl.obolibrary.org/obo/GAZ_00236579">
        <obo:RO_0001025 rdf:resource="http://purl.obolibrary.org/obo/GAZ_00015423"/>
        <obo:IAO_0000115>A fourth-level administrative division of Uganda.</obo:IAO_0000115>
        <oboInOwl:hasOBONamespace>GAZ</oboInOwl:hasOBONamespace>
        <oboInOwl:id>GAZ:00236579</oboInOwl:id>
        <rdfs:label>Sembabule Town</rdfs:label>
    </owl:NamedIndividual>
    


    <!-- http://purl.obolibrary.org/obo/GAZ_00236582 -->

    <owl:NamedIndividual rdf:about="http://purl.obolibrary.org/obo/GAZ_00236582">
        <obo:RO_0001025 rdf:resource="http://purl.obolibrary.org/obo/GAZ_00015414"/>
        <obo:IAO_0000115>A fourth-level administrative division of Uganda.</obo:IAO_0000115>
        <oboInOwl:hasOBONamespace>GAZ</oboInOwl:hasOBONamespace>
        <oboInOwl:id>GAZ:00236582</oboInOwl:id>
        <rdfs:label>Kakiri Sub-county</rdfs:label>
    </owl:NamedIndividual>
    


    <!-- http://purl.obolibrary.org/obo/GAZ_00236583 -->

    <owl:NamedIndividual rdf:about="http://purl.obolibrary.org/obo/GAZ_00236583">
        <obo:RO_0001025 rdf:resource="http://purl.obolibrary.org/obo/GAZ_00015414"/>
        <obo:IAO_0000115>A fourth-level administrative division of Uganda.</obo:IAO_0000115>
        <oboInOwl:hasOBONamespace>GAZ</oboInOwl:hasOBONamespace>
        <oboInOwl:id>GAZ:00236583</oboInOwl:id>
        <rdfs:label>Kasanje Sub-county</rdfs:label>
    </owl:NamedIndividual>
    


    <!-- http://purl.obolibrary.org/obo/GAZ_00236584 -->

    <owl:NamedIndividual rdf:about="http://purl.obolibrary.org/obo/GAZ_00236584">
        <obo:RO_0001025 rdf:resource="http://purl.obolibrary.org/obo/GAZ_00015414"/>
        <obo:IAO_0000115>A fourth-level administrative division of Uganda.</obo:IAO_0000115>
        <oboInOwl:hasOBONamespace>GAZ</oboInOwl:hasOBONamespace>
        <oboInOwl:id>GAZ:00236584</oboInOwl:id>
        <rdfs:label>Katabi Sub-county</rdfs:label>
    </owl:NamedIndividual>
    


    <!-- http://purl.obolibrary.org/obo/GAZ_00236585 -->

    <owl:NamedIndividual rdf:about="http://purl.obolibrary.org/obo/GAZ_00236585">
        <obo:RO_0001025 rdf:resource="http://purl.obolibrary.org/obo/GAZ_00015414"/>
        <obo:IAO_0000115>A fourth-level administrative division of Uganda.</obo:IAO_0000115>
        <oboInOwl:hasOBONamespace>GAZ</oboInOwl:hasOBONamespace>
        <oboInOwl:id>GAZ:00236585</oboInOwl:id>
        <rdfs:label>Masulita Sub-county</rdfs:label>
    </owl:NamedIndividual>
    


    <!-- http://purl.obolibrary.org/obo/GAZ_00236586 -->

    <owl:NamedIndividual rdf:about="http://purl.obolibrary.org/obo/GAZ_00236586">
        <obo:RO_0001025 rdf:resource="http://purl.obolibrary.org/obo/GAZ_00015414"/>
        <obo:IAO_0000115>A fourth-level administrative division of Uganda.</obo:IAO_0000115>
        <oboInOwl:hasOBONamespace>GAZ</oboInOwl:hasOBONamespace>
        <oboInOwl:id>GAZ:00236586</oboInOwl:id>
        <rdfs:label>Namayumba Sub-county</rdfs:label>
    </owl:NamedIndividual>
    


    <!-- http://purl.obolibrary.org/obo/GAZ_00236587 -->

    <owl:NamedIndividual rdf:about="http://purl.obolibrary.org/obo/GAZ_00236587">
        <obo:RO_0001025 rdf:resource="http://purl.obolibrary.org/obo/GAZ_00015414"/>
        <obo:IAO_0000115>A fourth-level administrative division of Uganda.</obo:IAO_0000115>
        <oboInOwl:hasOBONamespace>GAZ</oboInOwl:hasOBONamespace>
        <oboInOwl:id>GAZ:00236587</oboInOwl:id>
        <rdfs:label>Nsangi Sub-county</rdfs:label>
    </owl:NamedIndividual>
    


    <!-- http://purl.obolibrary.org/obo/GAZ_00236588 -->

    <owl:NamedIndividual rdf:about="http://purl.obolibrary.org/obo/GAZ_00236588">
        <obo:RO_0001025 rdf:resource="http://purl.obolibrary.org/obo/GAZ_00015414"/>
        <obo:IAO_0000115>A fourth-level administrative division of Uganda.</obo:IAO_0000115>
        <oboInOwl:hasOBONamespace>GAZ</oboInOwl:hasOBONamespace>
        <oboInOwl:id>GAZ:00236588</oboInOwl:id>
        <rdfs:label>Ssisa Sub-county</rdfs:label>
    </owl:NamedIndividual>
    


    <!-- http://purl.obolibrary.org/obo/GAZ_00236589 -->

    <owl:NamedIndividual rdf:about="http://purl.obolibrary.org/obo/GAZ_00236589">
        <obo:RO_0001025 rdf:resource="http://purl.obolibrary.org/obo/GAZ_00015414"/>
        <obo:IAO_0000115>A fourth-level administrative division of Uganda.</obo:IAO_0000115>
        <oboInOwl:hasOBONamespace>GAZ</oboInOwl:hasOBONamespace>
        <oboInOwl:id>GAZ:00236589</oboInOwl:id>
        <rdfs:label>Wakiso Sub-county</rdfs:label>
    </owl:NamedIndividual>
    


    <!-- http://purl.obolibrary.org/obo/GAZ_00236590 -->

    <owl:NamedIndividual rdf:about="http://purl.obolibrary.org/obo/GAZ_00236590">
        <obo:RO_0001025 rdf:resource="http://purl.obolibrary.org/obo/GAZ_00015414"/>
        <obo:IAO_0000115>A fourth-level administrative division of Uganda.</obo:IAO_0000115>
        <oboInOwl:hasOBONamespace>GAZ</oboInOwl:hasOBONamespace>
        <oboInOwl:id>GAZ:00236590</oboInOwl:id>
        <rdfs:label>Wakiso Town</rdfs:label>
    </owl:NamedIndividual>
    


    <!-- http://purl.obolibrary.org/obo/GAZ_00236591 -->

    <owl:NamedIndividual rdf:about="http://purl.obolibrary.org/obo/GAZ_00236591">
        <obo:RO_0001025 rdf:resource="http://purl.obolibrary.org/obo/GAZ_00015412"/>
        <obo:IAO_0000115>A fourth-level administrative division of Uganda.</obo:IAO_0000115>
        <oboInOwl:hasOBONamespace>GAZ</oboInOwl:hasOBONamespace>
        <oboInOwl:id>GAZ:00236591</oboInOwl:id>
        <rdfs:label>Busukuma Sub-county</rdfs:label>
    </owl:NamedIndividual>
    


    <!-- http://purl.obolibrary.org/obo/GAZ_00236592 -->

    <owl:NamedIndividual rdf:about="http://purl.obolibrary.org/obo/GAZ_00236592">
        <obo:RO_0001025 rdf:resource="http://purl.obolibrary.org/obo/GAZ_00015412"/>
        <obo:IAO_0000115>A fourth-level administrative division of Uganda.</obo:IAO_0000115>
        <oboInOwl:hasOBONamespace>GAZ</oboInOwl:hasOBONamespace>
        <oboInOwl:id>GAZ:00236592</oboInOwl:id>
        <rdfs:label>Gombe Sub-county</rdfs:label>
    </owl:NamedIndividual>
    


    <!-- http://purl.obolibrary.org/obo/GAZ_00236593 -->

    <owl:NamedIndividual rdf:about="http://purl.obolibrary.org/obo/GAZ_00236593">
        <obo:RO_0001025 rdf:resource="http://purl.obolibrary.org/obo/GAZ_00015412"/>
        <obo:IAO_0000115>A fourth-level administrative division of Uganda.</obo:IAO_0000115>
        <oboInOwl:hasOBONamespace>GAZ</oboInOwl:hasOBONamespace>
        <oboInOwl:id>GAZ:00236593</oboInOwl:id>
        <rdfs:label>Kira Sub-county</rdfs:label>
    </owl:NamedIndividual>
    


    <!-- http://purl.obolibrary.org/obo/GAZ_00236594 -->

    <owl:NamedIndividual rdf:about="http://purl.obolibrary.org/obo/GAZ_00236594">
        <obo:RO_0001025 rdf:resource="http://purl.obolibrary.org/obo/GAZ_00015412"/>
        <obo:IAO_0000115>A fourth-level administrative division of Uganda.</obo:IAO_0000115>
        <oboInOwl:hasOBONamespace>GAZ</oboInOwl:hasOBONamespace>
        <oboInOwl:id>GAZ:00236594</oboInOwl:id>
        <rdfs:label>Nabweru Sub-county</rdfs:label>
    </owl:NamedIndividual>
    


    <!-- http://purl.obolibrary.org/obo/GAZ_00236595 -->

    <owl:NamedIndividual rdf:about="http://purl.obolibrary.org/obo/GAZ_00236595">
        <obo:RO_0001025 rdf:resource="http://purl.obolibrary.org/obo/GAZ_00015412"/>
        <obo:IAO_0000115>A fourth-level administrative division of Uganda.</obo:IAO_0000115>
        <oboInOwl:hasOBONamespace>GAZ</oboInOwl:hasOBONamespace>
        <oboInOwl:id>GAZ:00236595</oboInOwl:id>
        <rdfs:label>Nangabo Sub-county</rdfs:label>
    </owl:NamedIndividual>
    


    <!-- http://purl.obolibrary.org/obo/GAZ_00236596 -->

    <owl:NamedIndividual rdf:about="http://purl.obolibrary.org/obo/GAZ_00236596">
        <obo:RO_0001025 rdf:resource="http://purl.obolibrary.org/obo/GAZ_00015412"/>
        <obo:IAO_0000115>A fourth-level administrative division of Uganda.</obo:IAO_0000115>
        <oboInOwl:hasOBONamespace>GAZ</oboInOwl:hasOBONamespace>
        <oboInOwl:id>GAZ:00236596</oboInOwl:id>
        <rdfs:label>Ssabagabo-Makindye</rdfs:label>
    </owl:NamedIndividual>
    


    <!-- http://purl.obolibrary.org/obo/GAZ_00236597 -->

    <owl:NamedIndividual rdf:about="http://purl.obolibrary.org/obo/GAZ_00236597">
        <obo:RO_0001025 rdf:resource="http://purl.obolibrary.org/obo/GAZ_00040046"/>
        <obo:IAO_0000115>An island.</obo:IAO_0000115>
        <oboInOwl:hasOBONamespace>GAZ</oboInOwl:hasOBONamespace>
        <oboInOwl:id>GAZ:00236597</oboInOwl:id>
        <rdfs:label>Ngamba Island</rdfs:label>
    </owl:NamedIndividual>
    


    <!-- http://purl.obolibrary.org/obo/GAZ_00236598 -->

    <owl:NamedIndividual rdf:about="http://purl.obolibrary.org/obo/GAZ_00236598">
        <obo:RO_0001025 rdf:resource="http://purl.obolibrary.org/obo/GAZ_00040046"/>
        <obo:IAO_0000115>An island.</obo:IAO_0000115>
        <oboInOwl:hasOBONamespace>GAZ</oboInOwl:hasOBONamespace>
        <oboInOwl:id>GAZ:00236598</oboInOwl:id>
        <rdfs:label>Nsadzi Island</rdfs:label>
    </owl:NamedIndividual>
    


    <!-- http://purl.obolibrary.org/obo/GAZ_00236599 -->

    <owl:NamedIndividual rdf:about="http://purl.obolibrary.org/obo/GAZ_00236599">
        <obo:RO_0001025 rdf:resource="http://purl.obolibrary.org/obo/GAZ_00040046"/>
        <obo:IAO_0000115>An island.</obo:IAO_0000115>
        <oboInOwl:hasOBONamespace>GAZ</oboInOwl:hasOBONamespace>
        <oboInOwl:id>GAZ:00236599</oboInOwl:id>
        <rdfs:label>Bulago Island</rdfs:label>
    </owl:NamedIndividual>
    


    <!-- http://purl.obolibrary.org/obo/GAZ_00236600 -->

    <owl:NamedIndividual rdf:about="http://purl.obolibrary.org/obo/GAZ_00236600">
        <rdf:type rdf:resource="http://purl.obolibrary.org/obo/ENVO_00000856"/>
        <obo:RO_0001025 rdf:resource="http://purl.obolibrary.org/obo/GAZ_00015412"/>
        <obo:IAO_0000115>A municipality in Wakiso District in Central Uganda.</obo:IAO_0000115>
        <oboInOwl:hasOBONamespace>GAZ</oboInOwl:hasOBONamespace>
        <oboInOwl:id>GAZ:00236600</oboInOwl:id>
        <rdfs:label>Kira Town</rdfs:label>
    </owl:NamedIndividual>
    


    <!-- http://purl.obolibrary.org/obo/GAZ_00236601 -->

    <owl:NamedIndividual rdf:about="http://purl.obolibrary.org/obo/GAZ_00236601">
        <obo:RO_0001025 rdf:resource="http://purl.obolibrary.org/obo/GAZ_00236600"/>
        <obo:IAO_0000115>An administrative ward (township) of Kira.</obo:IAO_0000115>
        <oboInOwl:hasOBONamespace>GAZ</oboInOwl:hasOBONamespace>
        <oboInOwl:id>GAZ:00236601</oboInOwl:id>
        <rdfs:label>Bweyogerere Ward</rdfs:label>
    </owl:NamedIndividual>
    


    <!-- http://purl.obolibrary.org/obo/GAZ_00236602 -->

    <owl:NamedIndividual rdf:about="http://purl.obolibrary.org/obo/GAZ_00236602">
        <obo:RO_0001025 rdf:resource="http://purl.obolibrary.org/obo/GAZ_00236600"/>
        <obo:IAO_0000115>An administrative ward (township) of Kira.</obo:IAO_0000115>
        <oboInOwl:hasOBONamespace>GAZ</oboInOwl:hasOBONamespace>
        <oboInOwl:id>GAZ:00236602</oboInOwl:id>
        <rdfs:label>Kireka Ward</rdfs:label>
    </owl:NamedIndividual>
    


    <!-- http://purl.obolibrary.org/obo/GAZ_00236603 -->

    <owl:NamedIndividual rdf:about="http://purl.obolibrary.org/obo/GAZ_00236603">
        <obo:RO_0001025 rdf:resource="http://purl.obolibrary.org/obo/GAZ_00236600"/>
        <obo:IAO_0000115>An administrative ward (township) of Kira.</obo:IAO_0000115>
        <oboInOwl:hasOBONamespace>GAZ</oboInOwl:hasOBONamespace>
        <oboInOwl:id>GAZ:00236603</oboInOwl:id>
        <rdfs:label>Kirinnya Ward</rdfs:label>
    </owl:NamedIndividual>
    


    <!-- http://purl.obolibrary.org/obo/GAZ_00236604 -->

    <owl:NamedIndividual rdf:about="http://purl.obolibrary.org/obo/GAZ_00236604">
        <obo:RO_0001025 rdf:resource="http://purl.obolibrary.org/obo/GAZ_00236600"/>
        <obo:IAO_0000115>An administrative ward (township) of Kira.</obo:IAO_0000115>
        <oboInOwl:hasOBONamespace>GAZ</oboInOwl:hasOBONamespace>
        <oboInOwl:id>GAZ:00236604</oboInOwl:id>
        <rdfs:label>Kyaliwajjala Ward</rdfs:label>
    </owl:NamedIndividual>
    


    <!-- http://purl.obolibrary.org/obo/GAZ_00236605 -->

    <owl:NamedIndividual rdf:about="http://purl.obolibrary.org/obo/GAZ_00236605">
        <obo:RO_0001025 rdf:resource="http://purl.obolibrary.org/obo/GAZ_00236600"/>
        <obo:IAO_0000115>An administrative ward (township) of Kira.</obo:IAO_0000115>
        <oboInOwl:hasOBONamespace>GAZ</oboInOwl:hasOBONamespace>
        <oboInOwl:id>GAZ:00236605</oboInOwl:id>
        <rdfs:label>Kira Ward</rdfs:label>
    </owl:NamedIndividual>
    


    <!-- http://purl.obolibrary.org/obo/GAZ_00236606 -->

    <owl:NamedIndividual rdf:about="http://purl.obolibrary.org/obo/GAZ_00236606">
        <obo:RO_0001025 rdf:resource="http://purl.obolibrary.org/obo/GAZ_00236600"/>
        <obo:IAO_0000115>An administrative ward (township) of Kira.</obo:IAO_0000115>
        <oboInOwl:hasOBONamespace>GAZ</oboInOwl:hasOBONamespace>
        <oboInOwl:id>GAZ:00236606</oboInOwl:id>
        <rdfs:label>Kimwaanyi Ward</rdfs:label>
    </owl:NamedIndividual>
    


    <!-- http://purl.obolibrary.org/obo/GAZ_00236607 -->

    <owl:NamedIndividual rdf:about="http://purl.obolibrary.org/obo/GAZ_00236607">
        <obo:RO_0001025 rdf:resource="http://purl.obolibrary.org/obo/GAZ_00005376"/>
        <obo:IAO_0000115>A subregion of the Eastern Region of Uganda.</obo:IAO_0000115>
        <oboInOwl:hasOBONamespace>GAZ</oboInOwl:hasOBONamespace>
        <oboInOwl:id>GAZ:00236607</oboInOwl:id>
        <rdfs:label>Teso Subregion</rdfs:label>
    </owl:NamedIndividual>
    


    <!-- http://purl.obolibrary.org/obo/GAZ_00236608 -->

    <owl:NamedIndividual rdf:about="http://purl.obolibrary.org/obo/GAZ_00236608">
        <obo:RO_0001025 rdf:resource="http://purl.obolibrary.org/obo/GAZ_00005375"/>
        <obo:IAO_0000115>A region in north-western Uganda that consists of the districts of Koboko, Moyo, Yumbe, Arua, Nebbi and the now defunct Madi district.</obo:IAO_0000115>
        <oboInOwl:hasOBONamespace>GAZ</oboInOwl:hasOBONamespace>
        <oboInOwl:id>GAZ:00236608</oboInOwl:id>
        <rdfs:label>West Nile Subregion</rdfs:label>
    </owl:NamedIndividual>
    


    <!-- http://purl.obolibrary.org/obo/GAZ_00236609 -->

    <owl:NamedIndividual rdf:about="http://purl.obolibrary.org/obo/GAZ_00236609">
        <obo:RO_0001025 rdf:resource="http://purl.obolibrary.org/obo/GAZ_00005375"/>
        <obo:IAO_0000115>A region in Uganda that consists of Amolatar District, Apac District, Dokolo District, Lira District and Oyam District.</obo:IAO_0000115>
        <oboInOwl:hasOBONamespace>GAZ</oboInOwl:hasOBONamespace>
        <oboInOwl:id>GAZ:00236609</oboInOwl:id>
        <rdfs:label>Lango Subegion</rdfs:label>
    </owl:NamedIndividual>
    


    <!-- http://purl.obolibrary.org/obo/GAZ_00236610 -->

    <owl:NamedIndividual rdf:about="http://purl.obolibrary.org/obo/GAZ_00236610">
        <obo:RO_0001025 rdf:resource="http://purl.obolibrary.org/obo/GAZ_00015454"/>
        <obo:IAO_0000115>A fourth-level administrative division of Uganda.</obo:IAO_0000115>
        <oboInOwl:hasOBONamespace>GAZ</oboInOwl:hasOBONamespace>
        <oboInOwl:id>GAZ:00236610</oboInOwl:id>
        <rdfs:label>Abarilela Sub-county</rdfs:label>
    </owl:NamedIndividual>
    


    <!-- http://purl.obolibrary.org/obo/GAZ_00236611 -->

    <owl:NamedIndividual rdf:about="http://purl.obolibrary.org/obo/GAZ_00236611">
        <obo:RO_0001025 rdf:resource="http://purl.obolibrary.org/obo/GAZ_00015454"/>
        <obo:IAO_0000115>A fourth-level administrative division of Uganda.</obo:IAO_0000115>
        <oboInOwl:hasOBONamespace>GAZ</oboInOwl:hasOBONamespace>
        <oboInOwl:id>GAZ:00236611</oboInOwl:id>
        <rdfs:label>Asamuk Sub-county</rdfs:label>
    </owl:NamedIndividual>
    


    <!-- http://purl.obolibrary.org/obo/GAZ_00236612 -->

    <owl:NamedIndividual rdf:about="http://purl.obolibrary.org/obo/GAZ_00236612">
        <obo:RO_0001025 rdf:resource="http://purl.obolibrary.org/obo/GAZ_00015454"/>
        <obo:IAO_0000115>A fourth-level administrative division of Uganda.</obo:IAO_0000115>
        <oboInOwl:hasOBONamespace>GAZ</oboInOwl:hasOBONamespace>
        <oboInOwl:id>GAZ:00236612</oboInOwl:id>
        <rdfs:label>Kuju Sub-county</rdfs:label>
    </owl:NamedIndividual>
    


    <!-- http://purl.obolibrary.org/obo/GAZ_00236613 -->

    <owl:NamedIndividual rdf:about="http://purl.obolibrary.org/obo/GAZ_00236613">
        <obo:RO_0001025 rdf:resource="http://purl.obolibrary.org/obo/GAZ_00015454"/>
        <obo:IAO_0000115>A fourth-level administrative division of Uganda.</obo:IAO_0000115>
        <oboInOwl:hasOBONamespace>GAZ</oboInOwl:hasOBONamespace>
        <oboInOwl:id>GAZ:00236613</oboInOwl:id>
        <rdfs:label>Orungo Sub-county</rdfs:label>
    </owl:NamedIndividual>
    


    <!-- http://purl.obolibrary.org/obo/GAZ_00236614 -->

    <owl:NamedIndividual rdf:about="http://purl.obolibrary.org/obo/GAZ_00236614">
        <obo:RO_0001025 rdf:resource="http://purl.obolibrary.org/obo/GAZ_00015454"/>
        <obo:IAO_0000115>A fourth-level administrative division of Uganda.</obo:IAO_0000115>
        <oboInOwl:hasOBONamespace>GAZ</oboInOwl:hasOBONamespace>
        <oboInOwl:id>GAZ:00236614</oboInOwl:id>
        <rdfs:label>Wera Sub-county</rdfs:label>
    </owl:NamedIndividual>
    


    <!-- http://purl.obolibrary.org/obo/GAZ_00236615 -->

    <owl:NamedIndividual rdf:about="http://purl.obolibrary.org/obo/GAZ_00236615">
        <obo:RO_0001025 rdf:resource="http://purl.obolibrary.org/obo/GAZ_00015454"/>
        <obo:IAO_0000115>A fourth-level administrative division of Uganda.</obo:IAO_0000115>
        <oboInOwl:hasOBONamespace>GAZ</oboInOwl:hasOBONamespace>
        <oboInOwl:id>GAZ:00236615</oboInOwl:id>
        <rdfs:label>Morungatuny Sub-county</rdfs:label>
    </owl:NamedIndividual>
    


    <!-- http://purl.obolibrary.org/obo/GAZ_00236616 -->

    <owl:NamedIndividual rdf:about="http://purl.obolibrary.org/obo/GAZ_00236616">
        <obo:RO_0001025 rdf:resource="http://purl.obolibrary.org/obo/GAZ_00015455"/>
        <obo:IAO_0000115>A fourth-level administrative division of Uganda.</obo:IAO_0000115>
        <oboInOwl:hasOBONamespace>GAZ</oboInOwl:hasOBONamespace>
        <oboInOwl:id>GAZ:00236616</oboInOwl:id>
        <rdfs:label>Acowa Sub-county</rdfs:label>
    </owl:NamedIndividual>
    


    <!-- http://purl.obolibrary.org/obo/GAZ_00236617 -->

    <owl:NamedIndividual rdf:about="http://purl.obolibrary.org/obo/GAZ_00236617">
        <obo:RO_0001025 rdf:resource="http://purl.obolibrary.org/obo/GAZ_00015455"/>
        <obo:IAO_0000115>A fourth-level administrative division of Uganda.</obo:IAO_0000115>
        <oboInOwl:hasOBONamespace>GAZ</oboInOwl:hasOBONamespace>
        <oboInOwl:id>GAZ:00236617</oboInOwl:id>
        <rdfs:label>Kapelebyong Sub-county</rdfs:label>
    </owl:NamedIndividual>
    


    <!-- http://purl.obolibrary.org/obo/GAZ_00236618 -->

    <owl:NamedIndividual rdf:about="http://purl.obolibrary.org/obo/GAZ_00236618">
        <obo:RO_0001025 rdf:resource="http://purl.obolibrary.org/obo/GAZ_00015455"/>
        <obo:IAO_0000115>A fourth-level administrative division of Uganda.</obo:IAO_0000115>
        <oboInOwl:hasOBONamespace>GAZ</oboInOwl:hasOBONamespace>
        <oboInOwl:id>GAZ:00236618</oboInOwl:id>
        <rdfs:label>Obalanga Sub-county</rdfs:label>
    </owl:NamedIndividual>
    


    <!-- http://purl.obolibrary.org/obo/GAZ_00236619 -->

    <owl:NamedIndividual rdf:about="http://purl.obolibrary.org/obo/GAZ_00236619">
        <obo:IAO_0000115>A fourth-level administrative division of Uganda.</obo:IAO_0000115>
        <oboInOwl:hasOBONamespace>GAZ</oboInOwl:hasOBONamespace>
        <oboInOwl:id>GAZ:00236619</oboInOwl:id>
        <rdfs:label>Kapujan Sub-county</rdfs:label>
    </owl:NamedIndividual>
    


    <!-- http://purl.obolibrary.org/obo/GAZ_00236620 -->

    <owl:NamedIndividual rdf:about="http://purl.obolibrary.org/obo/GAZ_00236620">
        <obo:IAO_0000115>A fourth-level administrative division of Uganda.</obo:IAO_0000115>
        <oboInOwl:hasOBONamespace>GAZ</oboInOwl:hasOBONamespace>
        <oboInOwl:id>GAZ:00236620</oboInOwl:id>
        <rdfs:label>Katakwi Sub-county</rdfs:label>
    </owl:NamedIndividual>
    


    <!-- http://purl.obolibrary.org/obo/GAZ_00236621 -->

    <owl:NamedIndividual rdf:about="http://purl.obolibrary.org/obo/GAZ_00236621">
        <obo:IAO_0000115>A fourth-level administrative division of Uganda.</obo:IAO_0000115>
        <oboInOwl:hasOBONamespace>GAZ</oboInOwl:hasOBONamespace>
        <oboInOwl:id>GAZ:00236621</oboInOwl:id>
        <rdfs:label>Katakwi Town</rdfs:label>
    </owl:NamedIndividual>
    


    <!-- http://purl.obolibrary.org/obo/GAZ_00236622 -->

    <owl:NamedIndividual rdf:about="http://purl.obolibrary.org/obo/GAZ_00236622">
        <obo:IAO_0000115>A fourth-level administrative division of Uganda.</obo:IAO_0000115>
        <oboInOwl:hasOBONamespace>GAZ</oboInOwl:hasOBONamespace>
        <oboInOwl:id>GAZ:00236622</oboInOwl:id>
        <rdfs:label>Magoro Sub-county</rdfs:label>
    </owl:NamedIndividual>
    


    <!-- http://purl.obolibrary.org/obo/GAZ_00236623 -->

    <owl:NamedIndividual rdf:about="http://purl.obolibrary.org/obo/GAZ_00236623">
        <obo:IAO_0000115>A fourth-level administrative division of Uganda.</obo:IAO_0000115>
        <oboInOwl:hasOBONamespace>GAZ</oboInOwl:hasOBONamespace>
        <oboInOwl:id>GAZ:00236623</oboInOwl:id>
        <rdfs:label>Ngariam Sub-county</rdfs:label>
    </owl:NamedIndividual>
    


    <!-- http://purl.obolibrary.org/obo/GAZ_00236624 -->

    <owl:NamedIndividual rdf:about="http://purl.obolibrary.org/obo/GAZ_00236624">
        <obo:IAO_0000115>A fourth-level administrative division of Uganda.</obo:IAO_0000115>
        <oboInOwl:hasOBONamespace>GAZ</oboInOwl:hasOBONamespace>
        <oboInOwl:id>GAZ:00236624</oboInOwl:id>
        <rdfs:label>Toroma Sub-county</rdfs:label>
    </owl:NamedIndividual>
    


    <!-- http://purl.obolibrary.org/obo/GAZ_00236625 -->

    <owl:NamedIndividual rdf:about="http://purl.obolibrary.org/obo/GAZ_00236625">
        <obo:IAO_0000115>A fourth-level administrative division of Uganda.</obo:IAO_0000115>
        <oboInOwl:hasOBONamespace>GAZ</oboInOwl:hasOBONamespace>
        <oboInOwl:id>GAZ:00236625</oboInOwl:id>
        <rdfs:label>Usuk Sub-county</rdfs:label>
    </owl:NamedIndividual>
    


    <!-- http://purl.obolibrary.org/obo/GAZ_00236626 -->

    <owl:NamedIndividual rdf:about="http://purl.obolibrary.org/obo/GAZ_00236626">
        <obo:IAO_0000115>A fourth-level administrative division of Uganda.</obo:IAO_0000115>
        <oboInOwl:hasOBONamespace>GAZ</oboInOwl:hasOBONamespace>
        <oboInOwl:id>GAZ:00236626</oboInOwl:id>
        <rdfs:label>Ongongoja Sub-county</rdfs:label>
    </owl:NamedIndividual>
    


    <!-- http://purl.obolibrary.org/obo/GAZ_00236627 -->

    <owl:NamedIndividual rdf:about="http://purl.obolibrary.org/obo/GAZ_00236627">
        <obo:IAO_0000115>A fourth-level administrative division of Uganda.</obo:IAO_0000115>
        <oboInOwl:hasOBONamespace>GAZ</oboInOwl:hasOBONamespace>
        <oboInOwl:id>GAZ:00236627</oboInOwl:id>
        <rdfs:label>Omodoi Sub-county</rdfs:label>
    </owl:NamedIndividual>
    


    <!-- http://purl.obolibrary.org/obo/GAZ_00236628 -->

    <owl:NamedIndividual rdf:about="http://purl.obolibrary.org/obo/GAZ_00236628">
        <obo:RO_0001025 rdf:resource="http://purl.obolibrary.org/obo/GAZ_00015456"/>
        <obo:IAO_0000115>A fourth-level administrative division of Uganda.</obo:IAO_0000115>
        <oboInOwl:hasOBONamespace>GAZ</oboInOwl:hasOBONamespace>
        <oboInOwl:id>GAZ:00236628</oboInOwl:id>
        <rdfs:label>Budaka Sub-County</rdfs:label>
    </owl:NamedIndividual>
    


    <!-- http://purl.obolibrary.org/obo/GAZ_00236629 -->

    <owl:NamedIndividual rdf:about="http://purl.obolibrary.org/obo/GAZ_00236629">
        <obo:RO_0001025 rdf:resource="http://purl.obolibrary.org/obo/GAZ_00015456"/>
        <obo:IAO_0000115>A fourth-level administrative division of Uganda.</obo:IAO_0000115>
        <oboInOwl:hasOBONamespace>GAZ</oboInOwl:hasOBONamespace>
        <oboInOwl:id>GAZ:00236629</oboInOwl:id>
        <rdfs:label>Iki-Iki Sub-County</rdfs:label>
    </owl:NamedIndividual>
    


    <!-- http://purl.obolibrary.org/obo/GAZ_00236630 -->

    <owl:NamedIndividual rdf:about="http://purl.obolibrary.org/obo/GAZ_00236630">
        <obo:RO_0001025 rdf:resource="http://purl.obolibrary.org/obo/GAZ_00015456"/>
        <obo:IAO_0000115>A fourth-level administrative division of Uganda.</obo:IAO_0000115>
        <oboInOwl:hasOBONamespace>GAZ</oboInOwl:hasOBONamespace>
        <oboInOwl:id>GAZ:00236630</oboInOwl:id>
        <rdfs:label>Naboa Sub-County</rdfs:label>
    </owl:NamedIndividual>
    


    <!-- http://purl.obolibrary.org/obo/GAZ_00236631 -->

    <owl:NamedIndividual rdf:about="http://purl.obolibrary.org/obo/GAZ_00236631">
        <obo:RO_0001025 rdf:resource="http://purl.obolibrary.org/obo/GAZ_00015456"/>
        <obo:IAO_0000115>A fourth-level administrative division of Uganda.</obo:IAO_0000115>
        <oboInOwl:hasOBONamespace>GAZ</oboInOwl:hasOBONamespace>
        <oboInOwl:id>GAZ:00236631</oboInOwl:id>
        <rdfs:label>Lyama Sub-County</rdfs:label>
    </owl:NamedIndividual>
    


    <!-- http://purl.obolibrary.org/obo/GAZ_00236632 -->

    <owl:NamedIndividual rdf:about="http://purl.obolibrary.org/obo/GAZ_00236632">
        <obo:RO_0001025 rdf:resource="http://purl.obolibrary.org/obo/GAZ_00015456"/>
        <obo:IAO_0000115>A fourth-level administrative division of Uganda.</obo:IAO_0000115>
        <oboInOwl:hasOBONamespace>GAZ</oboInOwl:hasOBONamespace>
        <oboInOwl:id>GAZ:00236632</oboInOwl:id>
        <rdfs:label>Kaderuna Sub-County</rdfs:label>
    </owl:NamedIndividual>
    


    <!-- http://purl.obolibrary.org/obo/GAZ_00236633 -->

    <owl:NamedIndividual rdf:about="http://purl.obolibrary.org/obo/GAZ_00236633">
        <obo:RO_0001025 rdf:resource="http://purl.obolibrary.org/obo/GAZ_00015456"/>
        <obo:IAO_0000115>A fourth-level administrative division of Uganda.</obo:IAO_0000115>
        <oboInOwl:hasOBONamespace>GAZ</oboInOwl:hasOBONamespace>
        <oboInOwl:id>GAZ:00236633</oboInOwl:id>
        <rdfs:label>Kamonkoli Sub-County</rdfs:label>
    </owl:NamedIndividual>
    


    <!-- http://purl.obolibrary.org/obo/GAZ_00236634 -->

    <owl:NamedIndividual rdf:about="http://purl.obolibrary.org/obo/GAZ_00236634">
        <obo:RO_0001025 rdf:resource="http://purl.obolibrary.org/obo/GAZ_00015456"/>
        <obo:IAO_0000115>A fourth-level administrative division of Uganda.</obo:IAO_0000115>
        <oboInOwl:hasOBONamespace>GAZ</oboInOwl:hasOBONamespace>
        <oboInOwl:id>GAZ:00236634</oboInOwl:id>
        <rdfs:label>Kameruka Sub-County</rdfs:label>
    </owl:NamedIndividual>
    


    <!-- http://purl.obolibrary.org/obo/GAZ_00236635 -->

    <owl:NamedIndividual rdf:about="http://purl.obolibrary.org/obo/GAZ_00236635">
        <obo:RO_0001025 rdf:resource="http://purl.obolibrary.org/obo/GAZ_00015457"/>
        <obo:IAO_0000115>A fourth-level administrative division of Uganda.</obo:IAO_0000115>
        <oboInOwl:hasOBONamespace>GAZ</oboInOwl:hasOBONamespace>
        <oboInOwl:id>GAZ:00236635</oboInOwl:id>
        <rdfs:label>Butebo Sub-county</rdfs:label>
    </owl:NamedIndividual>
    


    <!-- http://purl.obolibrary.org/obo/GAZ_00236636 -->

    <owl:NamedIndividual rdf:about="http://purl.obolibrary.org/obo/GAZ_00236636">
        <obo:RO_0001025 rdf:resource="http://purl.obolibrary.org/obo/GAZ_00015457"/>
        <obo:IAO_0000115>A fourth-level administrative division of Uganda.</obo:IAO_0000115>
        <oboInOwl:hasOBONamespace>GAZ</oboInOwl:hasOBONamespace>
        <oboInOwl:id>GAZ:00236636</oboInOwl:id>
        <rdfs:label>Kabwangasi Sub-county</rdfs:label>
    </owl:NamedIndividual>
    


    <!-- http://purl.obolibrary.org/obo/GAZ_00236637 -->

    <owl:NamedIndividual rdf:about="http://purl.obolibrary.org/obo/GAZ_00236637">
        <obo:RO_0001025 rdf:resource="http://purl.obolibrary.org/obo/GAZ_00015457"/>
        <obo:IAO_0000115>A fourth-level administrative division of Uganda.</obo:IAO_0000115>
        <oboInOwl:hasOBONamespace>GAZ</oboInOwl:hasOBONamespace>
        <oboInOwl:id>GAZ:00236637</oboInOwl:id>
        <rdfs:label>Kakoro Sub-county</rdfs:label>
    </owl:NamedIndividual>
    


    <!-- http://purl.obolibrary.org/obo/GAZ_00236638 -->

    <owl:NamedIndividual rdf:about="http://purl.obolibrary.org/obo/GAZ_00236638">
        <obo:RO_0001025 rdf:resource="http://purl.obolibrary.org/obo/GAZ_00015457"/>
        <obo:IAO_0000115>A fourth-level administrative division of Uganda.</obo:IAO_0000115>
        <oboInOwl:hasOBONamespace>GAZ</oboInOwl:hasOBONamespace>
        <oboInOwl:id>GAZ:00236638</oboInOwl:id>
        <rdfs:label>Kibale Sub-county</rdfs:label>
    </owl:NamedIndividual>
    


    <!-- http://purl.obolibrary.org/obo/GAZ_00236639 -->

    <owl:NamedIndividual rdf:about="http://purl.obolibrary.org/obo/GAZ_00236639">
        <obo:RO_0001025 rdf:resource="http://purl.obolibrary.org/obo/GAZ_00015457"/>
        <obo:IAO_0000115>A fourth-level administrative division of Uganda.</obo:IAO_0000115>
        <oboInOwl:hasOBONamespace>GAZ</oboInOwl:hasOBONamespace>
        <oboInOwl:id>GAZ:00236639</oboInOwl:id>
        <rdfs:label>Petete Sub-county</rdfs:label>
    </owl:NamedIndividual>
    


    <!-- http://purl.obolibrary.org/obo/GAZ_00236640 -->

    <owl:NamedIndividual rdf:about="http://purl.obolibrary.org/obo/GAZ_00236640">
        <obo:IAO_0000115>A fourth-level administrative division of Uganda.</obo:IAO_0000115>
        <oboInOwl:hasOBONamespace>GAZ</oboInOwl:hasOBONamespace>
        <oboInOwl:id>GAZ:00236640</oboInOwl:id>
        <rdfs:label>Bukwa Sub-county</rdfs:label>
    </owl:NamedIndividual>
    


    <!-- http://purl.obolibrary.org/obo/GAZ_00236641 -->

    <owl:NamedIndividual rdf:about="http://purl.obolibrary.org/obo/GAZ_00236641">
        <obo:IAO_0000115>A fourth-level administrative division of Uganda.</obo:IAO_0000115>
        <oboInOwl:hasOBONamespace>GAZ</oboInOwl:hasOBONamespace>
        <oboInOwl:id>GAZ:00236641</oboInOwl:id>
        <rdfs:label>Chesower Sub-county</rdfs:label>
    </owl:NamedIndividual>
    


    <!-- http://purl.obolibrary.org/obo/GAZ_00236642 -->

    <owl:NamedIndividual rdf:about="http://purl.obolibrary.org/obo/GAZ_00236642">
        <obo:IAO_0000115>A fourth-level administrative division of Uganda.</obo:IAO_0000115>
        <oboInOwl:hasOBONamespace>GAZ</oboInOwl:hasOBONamespace>
        <oboInOwl:id>GAZ:00236642</oboInOwl:id>
        <rdfs:label>Kabei Sub-county</rdfs:label>
    </owl:NamedIndividual>
    


    <!-- http://purl.obolibrary.org/obo/GAZ_00236643 -->

    <owl:NamedIndividual rdf:about="http://purl.obolibrary.org/obo/GAZ_00236643">
        <obo:IAO_0000115>A fourth-level administrative division of Uganda.</obo:IAO_0000115>
        <oboInOwl:hasOBONamespace>GAZ</oboInOwl:hasOBONamespace>
        <oboInOwl:id>GAZ:00236643</oboInOwl:id>
        <rdfs:label>Suam Sub-county</rdfs:label>
    </owl:NamedIndividual>
    


    <!-- http://purl.obolibrary.org/obo/GAZ_00236644 -->

    <owl:NamedIndividual rdf:about="http://purl.obolibrary.org/obo/GAZ_00236644">
        <obo:IAO_0000115>A fourth-level administrative division of Uganda.</obo:IAO_0000115>
        <oboInOwl:hasOBONamespace>GAZ</oboInOwl:hasOBONamespace>
        <oboInOwl:id>GAZ:00236644</oboInOwl:id>
        <rdfs:label>Banda Sub-county</rdfs:label>
    </owl:NamedIndividual>
    


    <!-- http://purl.obolibrary.org/obo/GAZ_00236645 -->

    <owl:NamedIndividual rdf:about="http://purl.obolibrary.org/obo/GAZ_00236645">
        <obo:IAO_0000115>A fourth-level administrative division of Uganda.</obo:IAO_0000115>
        <oboInOwl:hasOBONamespace>GAZ</oboInOwl:hasOBONamespace>
        <oboInOwl:id>GAZ:00236645</oboInOwl:id>
        <rdfs:label>Budhaya Sub-county</rdfs:label>
    </owl:NamedIndividual>
    


    <!-- http://purl.obolibrary.org/obo/GAZ_00236646 -->

    <owl:NamedIndividual rdf:about="http://purl.obolibrary.org/obo/GAZ_00236646">
        <obo:IAO_0000115>A fourth-level administrative division of Uganda.</obo:IAO_0000115>
        <oboInOwl:hasOBONamespace>GAZ</oboInOwl:hasOBONamespace>
        <oboInOwl:id>GAZ:00236646</oboInOwl:id>
        <rdfs:label>Bugiri Town</rdfs:label>
    </owl:NamedIndividual>
    


    <!-- http://purl.obolibrary.org/obo/GAZ_00236647 -->

    <owl:NamedIndividual rdf:about="http://purl.obolibrary.org/obo/GAZ_00236647">
        <obo:IAO_0000115>A fourth-level administrative division of Uganda.</obo:IAO_0000115>
        <oboInOwl:hasOBONamespace>GAZ</oboInOwl:hasOBONamespace>
        <oboInOwl:id>GAZ:00236647</oboInOwl:id>
        <rdfs:label>Bulesa Sub-county</rdfs:label>
    </owl:NamedIndividual>
    


    <!-- http://purl.obolibrary.org/obo/GAZ_00236648 -->

    <owl:NamedIndividual rdf:about="http://purl.obolibrary.org/obo/GAZ_00236648">
        <obo:IAO_0000115>A fourth-level administrative division of Uganda.</obo:IAO_0000115>
        <oboInOwl:hasOBONamespace>GAZ</oboInOwl:hasOBONamespace>
        <oboInOwl:id>GAZ:00236648</oboInOwl:id>
        <rdfs:label>Bulidha Sub-county</rdfs:label>
    </owl:NamedIndividual>
    


    <!-- http://purl.obolibrary.org/obo/GAZ_00236649 -->

    <owl:NamedIndividual rdf:about="http://purl.obolibrary.org/obo/GAZ_00236649">
        <obo:IAO_0000115>A fourth-level administrative division of Uganda.</obo:IAO_0000115>
        <oboInOwl:hasOBONamespace>GAZ</oboInOwl:hasOBONamespace>
        <oboInOwl:id>GAZ:00236649</oboInOwl:id>
        <rdfs:label>Buluguyi Sub-county</rdfs:label>
    </owl:NamedIndividual>
    


    <!-- http://purl.obolibrary.org/obo/GAZ_00236650 -->

    <owl:NamedIndividual rdf:about="http://purl.obolibrary.org/obo/GAZ_00236650">
        <obo:IAO_0000115>A fourth-level administrative division of Uganda.</obo:IAO_0000115>
        <oboInOwl:hasOBONamespace>GAZ</oboInOwl:hasOBONamespace>
        <oboInOwl:id>GAZ:00236650</oboInOwl:id>
        <rdfs:label>Buswale Sub-county</rdfs:label>
    </owl:NamedIndividual>
    


    <!-- http://purl.obolibrary.org/obo/GAZ_00236651 -->

    <owl:NamedIndividual rdf:about="http://purl.obolibrary.org/obo/GAZ_00236651">
        <obo:IAO_0000115>A fourth-level administrative division of Uganda.</obo:IAO_0000115>
        <oboInOwl:hasOBONamespace>GAZ</oboInOwl:hasOBONamespace>
        <oboInOwl:id>GAZ:00236651</oboInOwl:id>
        <rdfs:label>Buwunga Sub-county</rdfs:label>
    </owl:NamedIndividual>
    


    <!-- http://purl.obolibrary.org/obo/GAZ_00236652 -->

    <owl:NamedIndividual rdf:about="http://purl.obolibrary.org/obo/GAZ_00236652">
        <obo:IAO_0000115>A fourth-level administrative division of Uganda.</obo:IAO_0000115>
        <oboInOwl:hasOBONamespace>GAZ</oboInOwl:hasOBONamespace>
        <oboInOwl:id>GAZ:00236652</oboInOwl:id>
        <rdfs:label>Buyinja Sub-county</rdfs:label>
    </owl:NamedIndividual>
    


    <!-- http://purl.obolibrary.org/obo/GAZ_00236653 -->

    <owl:NamedIndividual rdf:about="http://purl.obolibrary.org/obo/GAZ_00236653">
        <obo:IAO_0000115>A fourth-level administrative division of Uganda.</obo:IAO_0000115>
        <oboInOwl:hasOBONamespace>GAZ</oboInOwl:hasOBONamespace>
        <oboInOwl:id>GAZ:00236653</oboInOwl:id>
        <rdfs:label>Iwemba Sub-county</rdfs:label>
    </owl:NamedIndividual>
    


    <!-- http://purl.obolibrary.org/obo/GAZ_00236654 -->

    <owl:NamedIndividual rdf:about="http://purl.obolibrary.org/obo/GAZ_00236654">
        <obo:IAO_0000115>A fourth-level administrative division of Uganda.</obo:IAO_0000115>
        <oboInOwl:hasOBONamespace>GAZ</oboInOwl:hasOBONamespace>
        <oboInOwl:id>GAZ:00236654</oboInOwl:id>
        <rdfs:label>Kapyanga Sub-county</rdfs:label>
    </owl:NamedIndividual>
    


    <!-- http://purl.obolibrary.org/obo/GAZ_00236655 -->

    <owl:NamedIndividual rdf:about="http://purl.obolibrary.org/obo/GAZ_00236655">
        <obo:IAO_0000115>A fourth-level administrative division of Uganda.</obo:IAO_0000115>
        <oboInOwl:hasOBONamespace>GAZ</oboInOwl:hasOBONamespace>
        <oboInOwl:id>GAZ:00236655</oboInOwl:id>
        <rdfs:label>Muterere Sub-county</rdfs:label>
    </owl:NamedIndividual>
    


    <!-- http://purl.obolibrary.org/obo/GAZ_00236656 -->

    <owl:NamedIndividual rdf:about="http://purl.obolibrary.org/obo/GAZ_00236656">
        <obo:IAO_0000115>A fourth-level administrative division of Uganda.</obo:IAO_0000115>
        <oboInOwl:hasOBONamespace>GAZ</oboInOwl:hasOBONamespace>
        <oboInOwl:id>GAZ:00236656</oboInOwl:id>
        <rdfs:label>Nabukalu Sub-county</rdfs:label>
    </owl:NamedIndividual>
    


    <!-- http://purl.obolibrary.org/obo/GAZ_00236657 -->

    <owl:NamedIndividual rdf:about="http://purl.obolibrary.org/obo/GAZ_00236657">
        <obo:IAO_0000115>A fourth-level administrative division of Uganda.</obo:IAO_0000115>
        <oboInOwl:hasOBONamespace>GAZ</oboInOwl:hasOBONamespace>
        <oboInOwl:id>GAZ:00236657</oboInOwl:id>
        <rdfs:label>Nankoma Sub-county</rdfs:label>
    </owl:NamedIndividual>
    


    <!-- http://purl.obolibrary.org/obo/GAZ_00236658 -->

    <owl:NamedIndividual rdf:about="http://purl.obolibrary.org/obo/GAZ_00236658">
        <obo:IAO_0000115>A fourth-level administrative division of Uganda.</obo:IAO_0000115>
        <oboInOwl:hasOBONamespace>GAZ</oboInOwl:hasOBONamespace>
        <oboInOwl:id>GAZ:00236658</oboInOwl:id>
        <rdfs:label>Sigulu Islands Sub-county</rdfs:label>
    </owl:NamedIndividual>
    


    <!-- http://purl.obolibrary.org/obo/GAZ_00236659 -->

    <owl:NamedIndividual rdf:about="http://purl.obolibrary.org/obo/GAZ_00236659">
        <obo:IAO_0000115>A fourth-level administrative division of Uganda.</obo:IAO_0000115>
        <oboInOwl:hasOBONamespace>GAZ</oboInOwl:hasOBONamespace>
        <oboInOwl:id>GAZ:00236659</oboInOwl:id>
        <rdfs:label>Mutumba Sub-county</rdfs:label>
    </owl:NamedIndividual>
    


    <!-- http://purl.obolibrary.org/obo/GAZ_00236660 -->

    <owl:NamedIndividual rdf:about="http://purl.obolibrary.org/obo/GAZ_00236660">
        <obo:RO_0001025 rdf:resource="http://purl.obolibrary.org/obo/GAZ_00015364"/>
        <obo:IAO_0000115>An administrative subdivision of Bududa District.</obo:IAO_0000115>
        <oboInOwl:hasOBONamespace>GAZ</oboInOwl:hasOBONamespace>
        <oboInOwl:id>GAZ:00236660</oboInOwl:id>
        <rdfs:label>Bukalasi Sub-county</rdfs:label>
    </owl:NamedIndividual>
    


    <!-- http://purl.obolibrary.org/obo/GAZ_00236661 -->

    <owl:NamedIndividual rdf:about="http://purl.obolibrary.org/obo/GAZ_00236661">
        <obo:RO_0001025 rdf:resource="http://purl.obolibrary.org/obo/GAZ_00015364"/>
        <obo:IAO_0000115>An administrative subdivision of Bududa District.</obo:IAO_0000115>
        <oboInOwl:hasOBONamespace>GAZ</oboInOwl:hasOBONamespace>
        <oboInOwl:id>GAZ:00236661</oboInOwl:id>
        <rdfs:label>Bukhabusi Sub-county</rdfs:label>
    </owl:NamedIndividual>
    


    <!-- http://purl.obolibrary.org/obo/GAZ_00236662 -->

    <owl:NamedIndividual rdf:about="http://purl.obolibrary.org/obo/GAZ_00236662">
        <obo:RO_0001025 rdf:resource="http://purl.obolibrary.org/obo/GAZ_00015364"/>
        <obo:IAO_0000115>An administrative subdivision of Bududa District.</obo:IAO_0000115>
        <oboInOwl:hasOBONamespace>GAZ</oboInOwl:hasOBONamespace>
        <oboInOwl:id>GAZ:00236662</oboInOwl:id>
        <rdfs:label>Bumboli Sub-county</rdfs:label>
    </owl:NamedIndividual>
    


    <!-- http://purl.obolibrary.org/obo/GAZ_00236663 -->

    <owl:NamedIndividual rdf:about="http://purl.obolibrary.org/obo/GAZ_00236663">
        <obo:RO_0001025 rdf:resource="http://purl.obolibrary.org/obo/GAZ_00015364"/>
        <obo:IAO_0000115>An administrative subdivision of Bududa District.</obo:IAO_0000115>
        <oboInOwl:hasOBONamespace>GAZ</oboInOwl:hasOBONamespace>
        <oboInOwl:id>GAZ:00236663</oboInOwl:id>
        <rdfs:label>Bubungi Sub-county</rdfs:label>
    </owl:NamedIndividual>
    


    <!-- http://purl.obolibrary.org/obo/GAZ_00236664 -->

    <owl:NamedIndividual rdf:about="http://purl.obolibrary.org/obo/GAZ_00236664">
        <obo:RO_0001025 rdf:resource="http://purl.obolibrary.org/obo/GAZ_00015364"/>
        <obo:IAO_0000115>An administrative subdivision of Bududa District.</obo:IAO_0000115>
        <oboInOwl:hasOBONamespace>GAZ</oboInOwl:hasOBONamespace>
        <oboInOwl:id>GAZ:00236664</oboInOwl:id>
        <rdfs:label>Khabutola Sub-county</rdfs:label>
    </owl:NamedIndividual>
    


    <!-- http://purl.obolibrary.org/obo/GAZ_00236665 -->

    <owl:NamedIndividual rdf:about="http://purl.obolibrary.org/obo/GAZ_00236665">
        <obo:RO_0001025 rdf:resource="http://purl.obolibrary.org/obo/GAZ_00015364"/>
        <obo:IAO_0000115>An administrative subdivision of Bududa District.</obo:IAO_0000115>
        <oboInOwl:hasOBONamespace>GAZ</oboInOwl:hasOBONamespace>
        <oboInOwl:id>GAZ:00236665</oboInOwl:id>
        <rdfs:label>Lukhonge Sub-county</rdfs:label>
    </owl:NamedIndividual>
    


    <!-- http://purl.obolibrary.org/obo/GAZ_00236666 -->

    <owl:NamedIndividual rdf:about="http://purl.obolibrary.org/obo/GAZ_00236666">
        <obo:RO_0001025 rdf:resource="http://purl.obolibrary.org/obo/GAZ_00015364"/>
        <obo:IAO_0000115>An administrative subdivision of Bududa District.</obo:IAO_0000115>
        <oboInOwl:hasOBONamespace>GAZ</oboInOwl:hasOBONamespace>
        <oboInOwl:id>GAZ:00236666</oboInOwl:id>
        <rdfs:label>Mayenze Sub-county</rdfs:label>
    </owl:NamedIndividual>
    


    <!-- http://purl.obolibrary.org/obo/GAZ_00236667 -->

    <owl:NamedIndividual rdf:about="http://purl.obolibrary.org/obo/GAZ_00236667">
        <obo:RO_0001025 rdf:resource="http://purl.obolibrary.org/obo/GAZ_00015364"/>
        <obo:IAO_0000115>An administrative subdivision of Bududa District.</obo:IAO_0000115>
        <oboInOwl:hasOBONamespace>GAZ</oboInOwl:hasOBONamespace>
        <oboInOwl:id>GAZ:00236667</oboInOwl:id>
        <rdfs:label>Bududa Town</rdfs:label>
    </owl:NamedIndividual>
    


    <!-- http://purl.obolibrary.org/obo/GAZ_00236668 -->

    <owl:NamedIndividual rdf:about="http://purl.obolibrary.org/obo/GAZ_00236668">
        <obo:IAO_0000115>A fourth-level administrative division of Uganda.</obo:IAO_0000115>
        <oboInOwl:hasOBONamespace>GAZ</oboInOwl:hasOBONamespace>
        <oboInOwl:id>GAZ:00236668</oboInOwl:id>
        <rdfs:label>Buhehe Sub-county</rdfs:label>
    </owl:NamedIndividual>
    


    <!-- http://purl.obolibrary.org/obo/GAZ_00236669 -->

    <owl:NamedIndividual rdf:about="http://purl.obolibrary.org/obo/GAZ_00236669">
        <obo:IAO_0000115>A fourth-level administrative division of Uganda.</obo:IAO_0000115>
        <oboInOwl:hasOBONamespace>GAZ</oboInOwl:hasOBONamespace>
        <oboInOwl:id>GAZ:00236669</oboInOwl:id>
        <rdfs:label>Bulumbi Sub-county</rdfs:label>
    </owl:NamedIndividual>
    


    <!-- http://purl.obolibrary.org/obo/GAZ_00236670 -->

    <owl:NamedIndividual rdf:about="http://purl.obolibrary.org/obo/GAZ_00236670">
        <obo:IAO_0000115>A fourth-level administrative division of Uganda.</obo:IAO_0000115>
        <oboInOwl:hasOBONamespace>GAZ</oboInOwl:hasOBONamespace>
        <oboInOwl:id>GAZ:00236670</oboInOwl:id>
        <rdfs:label>Busia Town</rdfs:label>
    </owl:NamedIndividual>
    


    <!-- http://purl.obolibrary.org/obo/GAZ_00236671 -->

    <owl:NamedIndividual rdf:about="http://purl.obolibrary.org/obo/GAZ_00236671">
        <obo:IAO_0000115>A fourth-level administrative division of Uganda.</obo:IAO_0000115>
        <oboInOwl:hasOBONamespace>GAZ</oboInOwl:hasOBONamespace>
        <oboInOwl:id>GAZ:00236671</oboInOwl:id>
        <rdfs:label>Busitema Sub-county</rdfs:label>
    </owl:NamedIndividual>
    


    <!-- http://purl.obolibrary.org/obo/GAZ_00236672 -->

    <owl:NamedIndividual rdf:about="http://purl.obolibrary.org/obo/GAZ_00236672">
        <obo:IAO_0000115>A fourth-level administrative division of Uganda.</obo:IAO_0000115>
        <oboInOwl:hasOBONamespace>GAZ</oboInOwl:hasOBONamespace>
        <oboInOwl:id>GAZ:00236672</oboInOwl:id>
        <rdfs:label>Buteba Sub-county</rdfs:label>
    </owl:NamedIndividual>
    


    <!-- http://purl.obolibrary.org/obo/GAZ_00236673 -->

    <owl:NamedIndividual rdf:about="http://purl.obolibrary.org/obo/GAZ_00236673">
        <obo:IAO_0000115>A fourth-level administrative division of Uganda.</obo:IAO_0000115>
        <oboInOwl:hasOBONamespace>GAZ</oboInOwl:hasOBONamespace>
        <oboInOwl:id>GAZ:00236673</oboInOwl:id>
        <rdfs:label>Dabani Sub-county</rdfs:label>
    </owl:NamedIndividual>
    


    <!-- http://purl.obolibrary.org/obo/GAZ_00236674 -->

    <owl:NamedIndividual rdf:about="http://purl.obolibrary.org/obo/GAZ_00236674">
        <obo:IAO_0000115>A fourth-level administrative division of Uganda.</obo:IAO_0000115>
        <oboInOwl:hasOBONamespace>GAZ</oboInOwl:hasOBONamespace>
        <oboInOwl:id>GAZ:00236674</oboInOwl:id>
        <rdfs:label>Lumino Sub-county</rdfs:label>
    </owl:NamedIndividual>
    


    <!-- http://purl.obolibrary.org/obo/GAZ_00236675 -->

    <owl:NamedIndividual rdf:about="http://purl.obolibrary.org/obo/GAZ_00236675">
        <obo:IAO_0000115>A fourth-level administrative division of Uganda.</obo:IAO_0000115>
        <oboInOwl:hasOBONamespace>GAZ</oboInOwl:hasOBONamespace>
        <oboInOwl:id>GAZ:00236675</oboInOwl:id>
        <rdfs:label>Lunyo Sub-county</rdfs:label>
    </owl:NamedIndividual>
    


    <!-- http://purl.obolibrary.org/obo/GAZ_00236676 -->

    <owl:NamedIndividual rdf:about="http://purl.obolibrary.org/obo/GAZ_00236676">
        <obo:IAO_0000115>A fourth-level administrative division of Uganda.</obo:IAO_0000115>
        <oboInOwl:hasOBONamespace>GAZ</oboInOwl:hasOBONamespace>
        <oboInOwl:id>GAZ:00236676</oboInOwl:id>
        <rdfs:label>Masaba Sub-county</rdfs:label>
    </owl:NamedIndividual>
    


    <!-- http://purl.obolibrary.org/obo/GAZ_00236677 -->

    <owl:NamedIndividual rdf:about="http://purl.obolibrary.org/obo/GAZ_00236677">
        <obo:IAO_0000115>A fourth-level administrative division of Uganda.</obo:IAO_0000115>
        <oboInOwl:hasOBONamespace>GAZ</oboInOwl:hasOBONamespace>
        <oboInOwl:id>GAZ:00236677</oboInOwl:id>
        <rdfs:label>Masafu Sub-county</rdfs:label>
    </owl:NamedIndividual>
    


    <!-- http://purl.obolibrary.org/obo/GAZ_00236678 -->

    <owl:NamedIndividual rdf:about="http://purl.obolibrary.org/obo/GAZ_00236678">
        <obo:IAO_0000115>A fourth-level administrative division of Uganda.</obo:IAO_0000115>
        <oboInOwl:hasOBONamespace>GAZ</oboInOwl:hasOBONamespace>
        <oboInOwl:id>GAZ:00236678</oboInOwl:id>
        <rdfs:label>Budumba Sub-county</rdfs:label>
    </owl:NamedIndividual>
    


    <!-- http://purl.obolibrary.org/obo/GAZ_00236679 -->

    <owl:NamedIndividual rdf:about="http://purl.obolibrary.org/obo/GAZ_00236679">
        <obo:IAO_0000115>A fourth-level administrative division of Uganda.</obo:IAO_0000115>
        <oboInOwl:hasOBONamespace>GAZ</oboInOwl:hasOBONamespace>
        <oboInOwl:id>GAZ:00236679</oboInOwl:id>
        <rdfs:label>Busaba Sub-county</rdfs:label>
    </owl:NamedIndividual>
    


    <!-- http://purl.obolibrary.org/obo/GAZ_00236680 -->

    <owl:NamedIndividual rdf:about="http://purl.obolibrary.org/obo/GAZ_00236680">
        <obo:IAO_0000115>A fourth-level administrative division of Uganda.</obo:IAO_0000115>
        <oboInOwl:hasOBONamespace>GAZ</oboInOwl:hasOBONamespace>
        <oboInOwl:id>GAZ:00236680</oboInOwl:id>
        <rdfs:label>Busolwe Sub-county</rdfs:label>
    </owl:NamedIndividual>
    


    <!-- http://purl.obolibrary.org/obo/GAZ_00236681 -->

    <owl:NamedIndividual rdf:about="http://purl.obolibrary.org/obo/GAZ_00236681">
        <obo:IAO_0000115>A fourth-level administrative division of Uganda.</obo:IAO_0000115>
        <oboInOwl:hasOBONamespace>GAZ</oboInOwl:hasOBONamespace>
        <oboInOwl:id>GAZ:00236681</oboInOwl:id>
        <rdfs:label>Butaleja Sub-county</rdfs:label>
    </owl:NamedIndividual>
    


    <!-- http://purl.obolibrary.org/obo/GAZ_00236682 -->

    <owl:NamedIndividual rdf:about="http://purl.obolibrary.org/obo/GAZ_00236682">
        <obo:IAO_0000115>A fourth-level administrative division of Uganda.</obo:IAO_0000115>
        <oboInOwl:hasOBONamespace>GAZ</oboInOwl:hasOBONamespace>
        <oboInOwl:id>GAZ:00236682</oboInOwl:id>
        <rdfs:label>Kachonga Sub-county</rdfs:label>
    </owl:NamedIndividual>
    


    <!-- http://purl.obolibrary.org/obo/GAZ_00236683 -->

    <owl:NamedIndividual rdf:about="http://purl.obolibrary.org/obo/GAZ_00236683">
        <obo:IAO_0000115>A fourth-level administrative division of Uganda.</obo:IAO_0000115>
        <oboInOwl:hasOBONamespace>GAZ</oboInOwl:hasOBONamespace>
        <oboInOwl:id>GAZ:00236683</oboInOwl:id>
        <rdfs:label>Nawanjofu Sub-county</rdfs:label>
    </owl:NamedIndividual>
    


    <!-- http://purl.obolibrary.org/obo/GAZ_00236684 -->

    <owl:NamedIndividual rdf:about="http://purl.obolibrary.org/obo/GAZ_00236684">
        <obo:IAO_0000115>A fourth-level administrative division of Uganda.</obo:IAO_0000115>
        <oboInOwl:hasOBONamespace>GAZ</oboInOwl:hasOBONamespace>
        <oboInOwl:id>GAZ:00236684</oboInOwl:id>
        <rdfs:label>Nazimasa Sub-county</rdfs:label>
    </owl:NamedIndividual>
    


    <!-- http://purl.obolibrary.org/obo/GAZ_00236685 -->

    <owl:NamedIndividual rdf:about="http://purl.obolibrary.org/obo/GAZ_00236685">
        <obo:RO_0001025 rdf:resource="http://purl.obolibrary.org/obo/GAZ_00015462"/>
        <obo:IAO_0000115>A fourth-level administrative division of Uganda.</obo:IAO_0000115>
        <oboInOwl:hasOBONamespace>GAZ</oboInOwl:hasOBONamespace>
        <oboInOwl:id>GAZ:00236685</oboInOwl:id>
        <rdfs:label>Buyanga Sub-county</rdfs:label>
    </owl:NamedIndividual>
    


    <!-- http://purl.obolibrary.org/obo/GAZ_00236686 -->

    <owl:NamedIndividual rdf:about="http://purl.obolibrary.org/obo/GAZ_00236686">
        <obo:RO_0001025 rdf:resource="http://purl.obolibrary.org/obo/GAZ_00015462"/>
        <obo:IAO_0000115>A fourth-level administrative division of Uganda.</obo:IAO_0000115>
        <oboInOwl:hasOBONamespace>GAZ</oboInOwl:hasOBONamespace>
        <oboInOwl:id>GAZ:00236686</oboInOwl:id>
        <rdfs:label>Ibulanku Sub-county</rdfs:label>
    </owl:NamedIndividual>
    


    <!-- http://purl.obolibrary.org/obo/GAZ_00236687 -->

    <owl:NamedIndividual rdf:about="http://purl.obolibrary.org/obo/GAZ_00236687">
        <obo:RO_0001025 rdf:resource="http://purl.obolibrary.org/obo/GAZ_00015462"/>
        <obo:IAO_0000115>A fourth-level administrative division of Uganda.</obo:IAO_0000115>
        <oboInOwl:hasOBONamespace>GAZ</oboInOwl:hasOBONamespace>
        <oboInOwl:id>GAZ:00236687</oboInOwl:id>
        <rdfs:label>Makuutu Sub-county</rdfs:label>
    </owl:NamedIndividual>
    


    <!-- http://purl.obolibrary.org/obo/GAZ_00236688 -->

    <owl:NamedIndividual rdf:about="http://purl.obolibrary.org/obo/GAZ_00236688">
        <obo:RO_0001025 rdf:resource="http://purl.obolibrary.org/obo/GAZ_00015462"/>
        <obo:IAO_0000115>A fourth-level administrative division of Uganda.</obo:IAO_0000115>
        <oboInOwl:hasOBONamespace>GAZ</oboInOwl:hasOBONamespace>
        <oboInOwl:id>GAZ:00236688</oboInOwl:id>
        <rdfs:label>Namalemba Sub-county</rdfs:label>
    </owl:NamedIndividual>
    


    <!-- http://purl.obolibrary.org/obo/GAZ_00236689 -->

    <owl:NamedIndividual rdf:about="http://purl.obolibrary.org/obo/GAZ_00236689">
        <obo:RO_0001025 rdf:resource="http://purl.obolibrary.org/obo/GAZ_00015462"/>
        <obo:IAO_0000115>A fourth-level administrative division of Uganda.</obo:IAO_0000115>
        <oboInOwl:hasOBONamespace>GAZ</oboInOwl:hasOBONamespace>
        <oboInOwl:id>GAZ:00236689</oboInOwl:id>
        <rdfs:label>Busiki Sub-county</rdfs:label>
    </owl:NamedIndividual>
    


    <!-- http://purl.obolibrary.org/obo/GAZ_00236690 -->

    <owl:NamedIndividual rdf:about="http://purl.obolibrary.org/obo/GAZ_00236690">
        <obo:RO_0001025 rdf:resource="http://purl.obolibrary.org/obo/GAZ_00015462"/>
        <obo:IAO_0000115>A fourth-level administrative division of Uganda.</obo:IAO_0000115>
        <oboInOwl:hasOBONamespace>GAZ</oboInOwl:hasOBONamespace>
        <oboInOwl:id>GAZ:00236690</oboInOwl:id>
        <rdfs:label>Bulange Sub-county</rdfs:label>
    </owl:NamedIndividual>
    


    <!-- http://purl.obolibrary.org/obo/GAZ_00236691 -->

    <owl:NamedIndividual rdf:about="http://purl.obolibrary.org/obo/GAZ_00236691">
        <obo:RO_0001025 rdf:resource="http://purl.obolibrary.org/obo/GAZ_00015462"/>
        <obo:IAO_0000115>A fourth-level administrative division of Uganda.</obo:IAO_0000115>
        <oboInOwl:hasOBONamespace>GAZ</oboInOwl:hasOBONamespace>
        <oboInOwl:id>GAZ:00236691</oboInOwl:id>
        <rdfs:label>Ivukula Sub-county</rdfs:label>
    </owl:NamedIndividual>
    


    <!-- http://purl.obolibrary.org/obo/GAZ_00236692 -->

    <owl:NamedIndividual rdf:about="http://purl.obolibrary.org/obo/GAZ_00236692">
        <obo:RO_0001025 rdf:resource="http://purl.obolibrary.org/obo/GAZ_00015462"/>
        <obo:IAO_0000115>A fourth-level administrative division of Uganda.</obo:IAO_0000115>
        <oboInOwl:hasOBONamespace>GAZ</oboInOwl:hasOBONamespace>
        <oboInOwl:id>GAZ:00236692</oboInOwl:id>
        <rdfs:label>Kibaale Sub-county</rdfs:label>
    </owl:NamedIndividual>
    


    <!-- http://purl.obolibrary.org/obo/GAZ_00236693 -->

    <owl:NamedIndividual rdf:about="http://purl.obolibrary.org/obo/GAZ_00236693">
        <obo:RO_0001025 rdf:resource="http://purl.obolibrary.org/obo/GAZ_00015462"/>
        <obo:IAO_0000115>A fourth-level administrative division of Uganda.</obo:IAO_0000115>
        <oboInOwl:hasOBONamespace>GAZ</oboInOwl:hasOBONamespace>
        <oboInOwl:id>GAZ:00236693</oboInOwl:id>
        <rdfs:label>Magada Sub-county</rdfs:label>
    </owl:NamedIndividual>
    


    <!-- http://purl.obolibrary.org/obo/GAZ_00236694 -->

    <owl:NamedIndividual rdf:about="http://purl.obolibrary.org/obo/GAZ_00236694">
        <obo:RO_0001025 rdf:resource="http://purl.obolibrary.org/obo/GAZ_00015462"/>
        <obo:IAO_0000115>A fourth-level administrative division of Uganda.</obo:IAO_0000115>
        <oboInOwl:hasOBONamespace>GAZ</oboInOwl:hasOBONamespace>
        <oboInOwl:id>GAZ:00236694</oboInOwl:id>
        <rdfs:label>Namutumba Sub-county</rdfs:label>
    </owl:NamedIndividual>
    


    <!-- http://purl.obolibrary.org/obo/GAZ_00236695 -->

    <owl:NamedIndividual rdf:about="http://purl.obolibrary.org/obo/GAZ_00236695">
        <obo:RO_0001025 rdf:resource="http://purl.obolibrary.org/obo/GAZ_00015462"/>
        <obo:IAO_0000115>A fourth-level administrative division of Uganda.</obo:IAO_0000115>
        <oboInOwl:hasOBONamespace>GAZ</oboInOwl:hasOBONamespace>
        <oboInOwl:id>GAZ:00236695</oboInOwl:id>
        <rdfs:label>Nsinze Sub-county</rdfs:label>
    </owl:NamedIndividual>
    


    <!-- http://purl.obolibrary.org/obo/GAZ_00236696 -->

    <owl:NamedIndividual rdf:about="http://purl.obolibrary.org/obo/GAZ_00236696">
        <obo:RO_0001025 rdf:resource="http://purl.obolibrary.org/obo/GAZ_00015463"/>
        <obo:IAO_0000115>A fourth-level administrative division of Uganda.</obo:IAO_0000115>
        <oboInOwl:hasOBONamespace>GAZ</oboInOwl:hasOBONamespace>
        <oboInOwl:id>GAZ:00236696</oboInOwl:id>
        <rdfs:label>Bulamagi Sub-county</rdfs:label>
    </owl:NamedIndividual>
    


    <!-- http://purl.obolibrary.org/obo/GAZ_00236697 -->

    <owl:NamedIndividual rdf:about="http://purl.obolibrary.org/obo/GAZ_00236697">
        <obo:RO_0001025 rdf:resource="http://purl.obolibrary.org/obo/GAZ_00015463"/>
        <obo:IAO_0000115>A fourth-level administrative division of Uganda.</obo:IAO_0000115>
        <oboInOwl:hasOBONamespace>GAZ</oboInOwl:hasOBONamespace>
        <oboInOwl:id>GAZ:00236697</oboInOwl:id>
        <rdfs:label>Iganga Town</rdfs:label>
    </owl:NamedIndividual>
    


    <!-- http://purl.obolibrary.org/obo/GAZ_00236698 -->

    <owl:NamedIndividual rdf:about="http://purl.obolibrary.org/obo/GAZ_00236698">
        <obo:RO_0001025 rdf:resource="http://purl.obolibrary.org/obo/GAZ_00015463"/>
        <obo:IAO_0000115>A fourth-level administrative division of Uganda.</obo:IAO_0000115>
        <oboInOwl:hasOBONamespace>GAZ</oboInOwl:hasOBONamespace>
        <oboInOwl:id>GAZ:00236698</oboInOwl:id>
        <rdfs:label>Nabitende Sub-county</rdfs:label>
    </owl:NamedIndividual>
    


    <!-- http://purl.obolibrary.org/obo/GAZ_00236699 -->

    <owl:NamedIndividual rdf:about="http://purl.obolibrary.org/obo/GAZ_00236699">
        <obo:RO_0001025 rdf:resource="http://purl.obolibrary.org/obo/GAZ_00015463"/>
        <obo:IAO_0000115>A fourth-level administrative division of Uganda.</obo:IAO_0000115>
        <oboInOwl:hasOBONamespace>GAZ</oboInOwl:hasOBONamespace>
        <oboInOwl:id>GAZ:00236699</oboInOwl:id>
        <rdfs:label>Nakalama Sub-county</rdfs:label>
    </owl:NamedIndividual>
    


    <!-- http://purl.obolibrary.org/obo/GAZ_00236700 -->

    <owl:NamedIndividual rdf:about="http://purl.obolibrary.org/obo/GAZ_00236700">
        <obo:RO_0001025 rdf:resource="http://purl.obolibrary.org/obo/GAZ_00015463"/>
        <obo:IAO_0000115>A fourth-level administrative division of Uganda.</obo:IAO_0000115>
        <oboInOwl:hasOBONamespace>GAZ</oboInOwl:hasOBONamespace>
        <oboInOwl:id>GAZ:00236700</oboInOwl:id>
        <rdfs:label>Nakigo Sub-county</rdfs:label>
    </owl:NamedIndividual>
    


    <!-- http://purl.obolibrary.org/obo/GAZ_00236701 -->

    <owl:NamedIndividual rdf:about="http://purl.obolibrary.org/obo/GAZ_00236701">
        <obo:RO_0001025 rdf:resource="http://purl.obolibrary.org/obo/GAZ_00015463"/>
        <obo:IAO_0000115>A fourth-level administrative division of Uganda.</obo:IAO_0000115>
        <oboInOwl:hasOBONamespace>GAZ</oboInOwl:hasOBONamespace>
        <oboInOwl:id>GAZ:00236701</oboInOwl:id>
        <rdfs:label>Nambale Sub-county</rdfs:label>
    </owl:NamedIndividual>
    


    <!-- http://purl.obolibrary.org/obo/GAZ_00236702 -->

    <owl:NamedIndividual rdf:about="http://purl.obolibrary.org/obo/GAZ_00236702">
        <obo:RO_0001025 rdf:resource="http://purl.obolibrary.org/obo/GAZ_00015463"/>
        <obo:IAO_0000115>A fourth-level administrative division of Uganda.</obo:IAO_0000115>
        <oboInOwl:hasOBONamespace>GAZ</oboInOwl:hasOBONamespace>
        <oboInOwl:id>GAZ:00236702</oboInOwl:id>
        <rdfs:label>Namungalwe Sub-county</rdfs:label>
    </owl:NamedIndividual>
    


    <!-- http://purl.obolibrary.org/obo/GAZ_00236703 -->

    <owl:NamedIndividual rdf:about="http://purl.obolibrary.org/obo/GAZ_00236703">
        <obo:RO_0001025 rdf:resource="http://purl.obolibrary.org/obo/GAZ_00015463"/>
        <obo:IAO_0000115>A fourth-level administrative division of Uganda.</obo:IAO_0000115>
        <oboInOwl:hasOBONamespace>GAZ</oboInOwl:hasOBONamespace>
        <oboInOwl:id>GAZ:00236703</oboInOwl:id>
        <rdfs:label>Nawandala Sub-county</rdfs:label>
    </owl:NamedIndividual>
    


    <!-- http://purl.obolibrary.org/obo/GAZ_00236704 -->

    <owl:NamedIndividual rdf:about="http://purl.obolibrary.org/obo/GAZ_00236704">
        <obo:RO_0001025 rdf:resource="http://purl.obolibrary.org/obo/GAZ_00015464"/>
        <obo:IAO_0000115>A fourth-level administrative division of Uganda.</obo:IAO_0000115>
        <oboInOwl:hasOBONamespace>GAZ</oboInOwl:hasOBONamespace>
        <oboInOwl:id>GAZ:00236704</oboInOwl:id>
        <rdfs:label>Bukanga Sub-county</rdfs:label>
    </owl:NamedIndividual>
    


    <!-- http://purl.obolibrary.org/obo/GAZ_00236705 -->

    <owl:NamedIndividual rdf:about="http://purl.obolibrary.org/obo/GAZ_00236705">
        <obo:RO_0001025 rdf:resource="http://purl.obolibrary.org/obo/GAZ_00015464"/>
        <obo:IAO_0000115>A fourth-level administrative division of Uganda.</obo:IAO_0000115>
        <oboInOwl:hasOBONamespace>GAZ</oboInOwl:hasOBONamespace>
        <oboInOwl:id>GAZ:00236705</oboInOwl:id>
        <rdfs:label>Bukooma Sub-county</rdfs:label>
    </owl:NamedIndividual>
    


    <!-- http://purl.obolibrary.org/obo/GAZ_00236706 -->

    <owl:NamedIndividual rdf:about="http://purl.obolibrary.org/obo/GAZ_00236706">
        <obo:RO_0001025 rdf:resource="http://purl.obolibrary.org/obo/GAZ_00015464"/>
        <obo:IAO_0000115>A fourth-level administrative division of Uganda.</obo:IAO_0000115>
        <oboInOwl:hasOBONamespace>GAZ</oboInOwl:hasOBONamespace>
        <oboInOwl:id>GAZ:00236706</oboInOwl:id>
        <rdfs:label>Bulongo Sub-county</rdfs:label>
    </owl:NamedIndividual>
    


    <!-- http://purl.obolibrary.org/obo/GAZ_00236707 -->

    <owl:NamedIndividual rdf:about="http://purl.obolibrary.org/obo/GAZ_00236707">
        <obo:RO_0001025 rdf:resource="http://purl.obolibrary.org/obo/GAZ_00015464"/>
        <obo:IAO_0000115>A fourth-level administrative division of Uganda.</obo:IAO_0000115>
        <oboInOwl:hasOBONamespace>GAZ</oboInOwl:hasOBONamespace>
        <oboInOwl:id>GAZ:00236707</oboInOwl:id>
        <rdfs:label>Ikumbya Sub-county</rdfs:label>
    </owl:NamedIndividual>
    


    <!-- http://purl.obolibrary.org/obo/GAZ_00236708 -->

    <owl:NamedIndividual rdf:about="http://purl.obolibrary.org/obo/GAZ_00236708">
        <obo:RO_0001025 rdf:resource="http://purl.obolibrary.org/obo/GAZ_00015464"/>
        <obo:IAO_0000115>A fourth-level administrative division of Uganda.</obo:IAO_0000115>
        <oboInOwl:hasOBONamespace>GAZ</oboInOwl:hasOBONamespace>
        <oboInOwl:id>GAZ:00236708</oboInOwl:id>
        <rdfs:label>Irongo Sub-county</rdfs:label>
    </owl:NamedIndividual>
    


    <!-- http://purl.obolibrary.org/obo/GAZ_00236709 -->

    <owl:NamedIndividual rdf:about="http://purl.obolibrary.org/obo/GAZ_00236709">
        <obo:RO_0001025 rdf:resource="http://purl.obolibrary.org/obo/GAZ_00015464"/>
        <obo:IAO_0000115>A fourth-level administrative division of Uganda.</obo:IAO_0000115>
        <oboInOwl:hasOBONamespace>GAZ</oboInOwl:hasOBONamespace>
        <oboInOwl:id>GAZ:00236709</oboInOwl:id>
        <rdfs:label>Nawampiti Sub-county</rdfs:label>
    </owl:NamedIndividual>
    


    <!-- http://purl.obolibrary.org/obo/GAZ_00236710 -->

    <owl:NamedIndividual rdf:about="http://purl.obolibrary.org/obo/GAZ_00236710">
        <obo:RO_0001025 rdf:resource="http://purl.obolibrary.org/obo/GAZ_00015464"/>
        <obo:IAO_0000115>A fourth-level administrative division of Uganda.</obo:IAO_0000115>
        <oboInOwl:hasOBONamespace>GAZ</oboInOwl:hasOBONamespace>
        <oboInOwl:id>GAZ:00236710</oboInOwl:id>
        <rdfs:label>Waibuga Sub-county</rdfs:label>
    </owl:NamedIndividual>
    


    <!-- http://purl.obolibrary.org/obo/GAZ_00236711 -->

    <owl:NamedIndividual rdf:about="http://purl.obolibrary.org/obo/GAZ_00236711">
        <obo:RO_0001025 rdf:resource="http://purl.obolibrary.org/obo/GAZ_00015465"/>
        <obo:IAO_0000115>A fourth-level administrative division of Uganda.</obo:IAO_0000115>
        <oboInOwl:hasOBONamespace>GAZ</oboInOwl:hasOBONamespace>
        <oboInOwl:id>GAZ:00236711</oboInOwl:id>
        <rdfs:label>Busedde Sub-county</rdfs:label>
    </owl:NamedIndividual>
    


    <!-- http://purl.obolibrary.org/obo/GAZ_00236712 -->

    <owl:NamedIndividual rdf:about="http://purl.obolibrary.org/obo/GAZ_00236712">
        <obo:RO_0001025 rdf:resource="http://purl.obolibrary.org/obo/GAZ_00015465"/>
        <obo:IAO_0000115>A fourth-level administrative division of Uganda.</obo:IAO_0000115>
        <oboInOwl:hasOBONamespace>GAZ</oboInOwl:hasOBONamespace>
        <oboInOwl:id>GAZ:00236712</oboInOwl:id>
        <rdfs:label>Kakira Sub-county</rdfs:label>
    </owl:NamedIndividual>
    


    <!-- http://purl.obolibrary.org/obo/GAZ_00236713 -->

    <owl:NamedIndividual rdf:about="http://purl.obolibrary.org/obo/GAZ_00236713">
        <obo:RO_0001025 rdf:resource="http://purl.obolibrary.org/obo/GAZ_00015465"/>
        <obo:IAO_0000115>A fourth-level administrative division of Uganda.</obo:IAO_0000115>
        <oboInOwl:hasOBONamespace>GAZ</oboInOwl:hasOBONamespace>
        <oboInOwl:id>GAZ:00236713</oboInOwl:id>
        <rdfs:label>Mafubira Sub-county</rdfs:label>
    </owl:NamedIndividual>
    


    <!-- http://purl.obolibrary.org/obo/GAZ_00236714 -->

    <owl:NamedIndividual rdf:about="http://purl.obolibrary.org/obo/GAZ_00236714">
        <obo:RO_0001025 rdf:resource="http://purl.obolibrary.org/obo/GAZ_00015467"/>
        <obo:IAO_0000115>A fourth-level administrative division of Uganda.</obo:IAO_0000115>
        <oboInOwl:hasOBONamespace>GAZ</oboInOwl:hasOBONamespace>
        <oboInOwl:id>GAZ:00236714</oboInOwl:id>
        <rdfs:label>Budondo Sub-county</rdfs:label>
    </owl:NamedIndividual>
    


    <!-- http://purl.obolibrary.org/obo/GAZ_00236715 -->

    <owl:NamedIndividual rdf:about="http://purl.obolibrary.org/obo/GAZ_00236715">
        <obo:RO_0001025 rdf:resource="http://purl.obolibrary.org/obo/GAZ_00015467"/>
        <obo:IAO_0000115>A fourth-level administrative division of Uganda.</obo:IAO_0000115>
        <oboInOwl:hasOBONamespace>GAZ</oboInOwl:hasOBONamespace>
        <oboInOwl:id>GAZ:00236715</oboInOwl:id>
        <rdfs:label>Butagaya Sub-county</rdfs:label>
    </owl:NamedIndividual>
    


    <!-- http://purl.obolibrary.org/obo/GAZ_00236716 -->

    <owl:NamedIndividual rdf:about="http://purl.obolibrary.org/obo/GAZ_00236716">
        <obo:RO_0001025 rdf:resource="http://purl.obolibrary.org/obo/GAZ_00015467"/>
        <obo:IAO_0000115>A fourth-level administrative division of Uganda.</obo:IAO_0000115>
        <oboInOwl:hasOBONamespace>GAZ</oboInOwl:hasOBONamespace>
        <oboInOwl:id>GAZ:00236716</oboInOwl:id>
        <rdfs:label>Buwenge Sub-county</rdfs:label>
    </owl:NamedIndividual>
    


    <!-- http://purl.obolibrary.org/obo/GAZ_00236717 -->

    <owl:NamedIndividual rdf:about="http://purl.obolibrary.org/obo/GAZ_00236717">
        <obo:RO_0001025 rdf:resource="http://purl.obolibrary.org/obo/GAZ_00015467"/>
        <obo:IAO_0000115>A fourth-level administrative division of Uganda.</obo:IAO_0000115>
        <oboInOwl:hasOBONamespace>GAZ</oboInOwl:hasOBONamespace>
        <oboInOwl:id>GAZ:00236717</oboInOwl:id>
        <rdfs:label>Buwenge Town</rdfs:label>
    </owl:NamedIndividual>
    


    <!-- http://purl.obolibrary.org/obo/GAZ_00236718 -->

    <owl:NamedIndividual rdf:about="http://purl.obolibrary.org/obo/GAZ_00236718">
        <obo:RO_0001025 rdf:resource="http://purl.obolibrary.org/obo/GAZ_00015467"/>
        <obo:IAO_0000115>A fourth-level administrative division of Uganda.</obo:IAO_0000115>
        <oboInOwl:hasOBONamespace>GAZ</oboInOwl:hasOBONamespace>
        <oboInOwl:id>GAZ:00236718</oboInOwl:id>
        <rdfs:label>Buyengo Sub-county</rdfs:label>
    </owl:NamedIndividual>
    


    <!-- http://purl.obolibrary.org/obo/GAZ_00236719 -->

    <owl:NamedIndividual rdf:about="http://purl.obolibrary.org/obo/GAZ_00236719">
        <obo:RO_0001025 rdf:resource="http://purl.obolibrary.org/obo/GAZ_00015466"/>
        <obo:IAO_0000115>A fourth-level administrative division of Uganda.</obo:IAO_0000115>
        <oboInOwl:hasOBONamespace>GAZ</oboInOwl:hasOBONamespace>
        <oboInOwl:id>GAZ:00236719</oboInOwl:id>
        <rdfs:label>Jinga Central Division</rdfs:label>
    </owl:NamedIndividual>
    


    <!-- http://purl.obolibrary.org/obo/GAZ_00236720 -->

    <owl:NamedIndividual rdf:about="http://purl.obolibrary.org/obo/GAZ_00236720">
        <obo:RO_0001025 rdf:resource="http://purl.obolibrary.org/obo/GAZ_00015466"/>
        <obo:IAO_0000115>A fourth-level administrative division of Uganda.</obo:IAO_0000115>
        <oboInOwl:hasOBONamespace>GAZ</oboInOwl:hasOBONamespace>
        <oboInOwl:id>GAZ:00236720</oboInOwl:id>
        <rdfs:label>Mpumudde/Kimaka Division</rdfs:label>
    </owl:NamedIndividual>
    


    <!-- http://purl.obolibrary.org/obo/GAZ_00236721 -->

    <owl:NamedIndividual rdf:about="http://purl.obolibrary.org/obo/GAZ_00236721">
        <obo:RO_0001025 rdf:resource="http://purl.obolibrary.org/obo/GAZ_00015466"/>
        <obo:IAO_0000115>A fourth-level administrative division of Uganda.</obo:IAO_0000115>
        <oboInOwl:hasOBONamespace>GAZ</oboInOwl:hasOBONamespace>
        <oboInOwl:id>GAZ:00236721</oboInOwl:id>
        <rdfs:label>Masese/Walukuba Division</rdfs:label>
    </owl:NamedIndividual>
    


    <!-- http://purl.obolibrary.org/obo/GAZ_00236722 -->

    <owl:NamedIndividual rdf:about="http://purl.obolibrary.org/obo/GAZ_00236722">
        <obo:RO_0001025 rdf:resource="http://purl.obolibrary.org/obo/GAZ_00015468"/>
        <obo:IAO_0000115>A fourth-level administrative division of Uganda.</obo:IAO_0000115>
        <oboInOwl:hasOBONamespace>GAZ</oboInOwl:hasOBONamespace>
        <oboInOwl:id>GAZ:00236722</oboInOwl:id>
        <rdfs:label>Alwa Sub-county</rdfs:label>
    </owl:NamedIndividual>
    


    <!-- http://purl.obolibrary.org/obo/GAZ_00236723 -->

    <owl:NamedIndividual rdf:about="http://purl.obolibrary.org/obo/GAZ_00236723">
        <obo:RO_0001025 rdf:resource="http://purl.obolibrary.org/obo/GAZ_00015468"/>
        <obo:IAO_0000115>A fourth-level administrative division of Uganda.</obo:IAO_0000115>
        <oboInOwl:hasOBONamespace>GAZ</oboInOwl:hasOBONamespace>
        <oboInOwl:id>GAZ:00236723</oboInOwl:id>
        <rdfs:label>Kaberamaido Sub-county</rdfs:label>
    </owl:NamedIndividual>
    


    <!-- http://purl.obolibrary.org/obo/GAZ_00236724 -->

    <owl:NamedIndividual rdf:about="http://purl.obolibrary.org/obo/GAZ_00236724">
        <obo:RO_0001025 rdf:resource="http://purl.obolibrary.org/obo/GAZ_00015468"/>
        <obo:IAO_0000115>A fourth-level administrative division of Uganda.</obo:IAO_0000115>
        <oboInOwl:hasOBONamespace>GAZ</oboInOwl:hasOBONamespace>
        <oboInOwl:id>GAZ:00236724</oboInOwl:id>
        <rdfs:label>Kobulubulu Sub-county</rdfs:label>
    </owl:NamedIndividual>
    


    <!-- http://purl.obolibrary.org/obo/GAZ_00236725 -->

    <owl:NamedIndividual rdf:about="http://purl.obolibrary.org/obo/GAZ_00236725">
        <obo:RO_0001025 rdf:resource="http://purl.obolibrary.org/obo/GAZ_00015468"/>
        <obo:IAO_0000115>A fourth-level administrative division of Uganda.</obo:IAO_0000115>
        <oboInOwl:hasOBONamespace>GAZ</oboInOwl:hasOBONamespace>
        <oboInOwl:id>GAZ:00236725</oboInOwl:id>
        <rdfs:label>Ochero Sub-county</rdfs:label>
    </owl:NamedIndividual>
    


    <!-- http://purl.obolibrary.org/obo/GAZ_00236726 -->

    <owl:NamedIndividual rdf:about="http://purl.obolibrary.org/obo/GAZ_00236726">
        <obo:RO_0001025 rdf:resource="http://purl.obolibrary.org/obo/GAZ_00015468"/>
        <obo:IAO_0000115>A fourth-level administrative division of Uganda.</obo:IAO_0000115>
        <oboInOwl:hasOBONamespace>GAZ</oboInOwl:hasOBONamespace>
        <oboInOwl:id>GAZ:00236726</oboInOwl:id>
        <rdfs:label>Kaberamaido Town</rdfs:label>
    </owl:NamedIndividual>
    


    <!-- http://purl.obolibrary.org/obo/GAZ_00236727 -->

    <owl:NamedIndividual rdf:about="http://purl.obolibrary.org/obo/GAZ_00236727">
        <obo:RO_0001025 rdf:resource="http://purl.obolibrary.org/obo/GAZ_00015469"/>
        <obo:IAO_0000115>A fourth-level administrative division of Uganda.</obo:IAO_0000115>
        <oboInOwl:hasOBONamespace>GAZ</oboInOwl:hasOBONamespace>
        <oboInOwl:id>GAZ:00236727</oboInOwl:id>
        <rdfs:label>Anyara Sub-county</rdfs:label>
    </owl:NamedIndividual>
    


    <!-- http://purl.obolibrary.org/obo/GAZ_00236728 -->

    <owl:NamedIndividual rdf:about="http://purl.obolibrary.org/obo/GAZ_00236728">
        <obo:RO_0001025 rdf:resource="http://purl.obolibrary.org/obo/GAZ_00015469"/>
        <obo:IAO_0000115>A fourth-level administrative division of Uganda.</obo:IAO_0000115>
        <oboInOwl:hasOBONamespace>GAZ</oboInOwl:hasOBONamespace>
        <oboInOwl:id>GAZ:00236728</oboInOwl:id>
        <rdfs:label>Bululu Sub-county</rdfs:label>
    </owl:NamedIndividual>
    


    <!-- http://purl.obolibrary.org/obo/GAZ_00236729 -->

    <owl:NamedIndividual rdf:about="http://purl.obolibrary.org/obo/GAZ_00236729">
        <obo:RO_0001025 rdf:resource="http://purl.obolibrary.org/obo/GAZ_00015469"/>
        <obo:IAO_0000115>A fourth-level administrative division of Uganda.</obo:IAO_0000115>
        <oboInOwl:hasOBONamespace>GAZ</oboInOwl:hasOBONamespace>
        <oboInOwl:id>GAZ:00236729</oboInOwl:id>
        <rdfs:label>Kalaki Sub-county</rdfs:label>
    </owl:NamedIndividual>
    


    <!-- http://purl.obolibrary.org/obo/GAZ_00236730 -->

    <owl:NamedIndividual rdf:about="http://purl.obolibrary.org/obo/GAZ_00236730">
        <obo:RO_0001025 rdf:resource="http://purl.obolibrary.org/obo/GAZ_00015469"/>
        <obo:IAO_0000115>A fourth-level administrative division of Uganda.</obo:IAO_0000115>
        <oboInOwl:hasOBONamespace>GAZ</oboInOwl:hasOBONamespace>
        <oboInOwl:id>GAZ:00236730</oboInOwl:id>
        <rdfs:label>Otuboi Sub-county</rdfs:label>
    </owl:NamedIndividual>
    


    <!-- http://purl.obolibrary.org/obo/GAZ_00236731 -->

    <owl:NamedIndividual rdf:about="http://purl.obolibrary.org/obo/GAZ_00236731">
        <obo:RO_0001025 rdf:resource="http://purl.obolibrary.org/obo/GAZ_00015366"/>
        <obo:IAO_0000115>A fourth-level administrative division of Uganda.</obo:IAO_0000115>
        <oboInOwl:hasOBONamespace>GAZ</oboInOwl:hasOBONamespace>
        <oboInOwl:id>GAZ:00236731</oboInOwl:id>
        <rdfs:label>Bukedea Sub-county</rdfs:label>
    </owl:NamedIndividual>
    


    <!-- http://purl.obolibrary.org/obo/GAZ_00236732 -->

    <owl:NamedIndividual rdf:about="http://purl.obolibrary.org/obo/GAZ_00236732">
        <obo:RO_0001025 rdf:resource="http://purl.obolibrary.org/obo/GAZ_00015366"/>
        <obo:IAO_0000115>A fourth-level administrative division of Uganda.</obo:IAO_0000115>
        <oboInOwl:hasOBONamespace>GAZ</oboInOwl:hasOBONamespace>
        <oboInOwl:id>GAZ:00236732</oboInOwl:id>
        <rdfs:label>Kachumbala Sub-county</rdfs:label>
    </owl:NamedIndividual>
    


    <!-- http://purl.obolibrary.org/obo/GAZ_00236733 -->

    <owl:NamedIndividual rdf:about="http://purl.obolibrary.org/obo/GAZ_00236733">
        <obo:RO_0001025 rdf:resource="http://purl.obolibrary.org/obo/GAZ_00015366"/>
        <obo:IAO_0000115>A fourth-level administrative division of Uganda.</obo:IAO_0000115>
        <oboInOwl:hasOBONamespace>GAZ</oboInOwl:hasOBONamespace>
        <oboInOwl:id>GAZ:00236733</oboInOwl:id>
        <rdfs:label>Kidongole Sub-county</rdfs:label>
    </owl:NamedIndividual>
    


    <!-- http://purl.obolibrary.org/obo/GAZ_00236734 -->

    <owl:NamedIndividual rdf:about="http://purl.obolibrary.org/obo/GAZ_00236734">
        <obo:RO_0001025 rdf:resource="http://purl.obolibrary.org/obo/GAZ_00015366"/>
        <obo:IAO_0000115>A fourth-level administrative division of Uganda.</obo:IAO_0000115>
        <oboInOwl:hasOBONamespace>GAZ</oboInOwl:hasOBONamespace>
        <oboInOwl:id>GAZ:00236734</oboInOwl:id>
        <rdfs:label>Kolir Sub-county</rdfs:label>
    </owl:NamedIndividual>
    


    <!-- http://purl.obolibrary.org/obo/GAZ_00236735 -->

    <owl:NamedIndividual rdf:about="http://purl.obolibrary.org/obo/GAZ_00236735">
        <obo:RO_0001025 rdf:resource="http://purl.obolibrary.org/obo/GAZ_00015366"/>
        <obo:IAO_0000115>A fourth-level administrative division of Uganda.</obo:IAO_0000115>
        <oboInOwl:hasOBONamespace>GAZ</oboInOwl:hasOBONamespace>
        <oboInOwl:id>GAZ:00236735</oboInOwl:id>
        <rdfs:label>Malera Sub-county</rdfs:label>
    </owl:NamedIndividual>
    


    <!-- http://purl.obolibrary.org/obo/GAZ_00236736 -->

    <owl:NamedIndividual rdf:about="http://purl.obolibrary.org/obo/GAZ_00236736">
        <obo:RO_0001025 rdf:resource="http://purl.obolibrary.org/obo/GAZ_00015470"/>
        <obo:IAO_0000115>A fourth-level administrative division of Uganda.</obo:IAO_0000115>
        <oboInOwl:hasOBONamespace>GAZ</oboInOwl:hasOBONamespace>
        <oboInOwl:id>GAZ:00236736</oboInOwl:id>
        <rdfs:label>Bumanya Sub-county</rdfs:label>
    </owl:NamedIndividual>
    


    <!-- http://purl.obolibrary.org/obo/GAZ_00236737 -->

    <owl:NamedIndividual rdf:about="http://purl.obolibrary.org/obo/GAZ_00236737">
        <obo:RO_0001025 rdf:resource="http://purl.obolibrary.org/obo/GAZ_00015470"/>
        <obo:IAO_0000115>A fourth-level administrative division of Uganda.</obo:IAO_0000115>
        <oboInOwl:hasOBONamespace>GAZ</oboInOwl:hasOBONamespace>
        <oboInOwl:id>GAZ:00236737</oboInOwl:id>
        <rdfs:label>Gadumire Sub-county</rdfs:label>
    </owl:NamedIndividual>
    


    <!-- http://purl.obolibrary.org/obo/GAZ_00236738 -->

    <owl:NamedIndividual rdf:about="http://purl.obolibrary.org/obo/GAZ_00236738">
        <obo:RO_0001025 rdf:resource="http://purl.obolibrary.org/obo/GAZ_00015470"/>
        <obo:IAO_0000115>A fourth-level administrative division of Uganda.</obo:IAO_0000115>
        <oboInOwl:hasOBONamespace>GAZ</oboInOwl:hasOBONamespace>
        <oboInOwl:id>GAZ:00236738</oboInOwl:id>
        <rdfs:label>Namugongo Sub-county</rdfs:label>
    </owl:NamedIndividual>
    


    <!-- http://purl.obolibrary.org/obo/GAZ_00236739 -->

    <owl:NamedIndividual rdf:about="http://purl.obolibrary.org/obo/GAZ_00236739">
        <obo:RO_0001025 rdf:resource="http://purl.obolibrary.org/obo/GAZ_00015470"/>
        <obo:IAO_0000115>A fourth-level administrative division of Uganda.</obo:IAO_0000115>
        <oboInOwl:hasOBONamespace>GAZ</oboInOwl:hasOBONamespace>
        <oboInOwl:id>GAZ:00236739</oboInOwl:id>
        <rdfs:label>Namwiwa Sub-county</rdfs:label>
    </owl:NamedIndividual>
    


    <!-- http://purl.obolibrary.org/obo/GAZ_00236740 -->

    <owl:NamedIndividual rdf:about="http://purl.obolibrary.org/obo/GAZ_00236740">
        <obo:RO_0001025 rdf:resource="http://purl.obolibrary.org/obo/GAZ_00015470"/>
        <obo:IAO_0000115>A fourth-level administrative division of Uganda.</obo:IAO_0000115>
        <oboInOwl:hasOBONamespace>GAZ</oboInOwl:hasOBONamespace>
        <oboInOwl:id>GAZ:00236740</oboInOwl:id>
        <rdfs:label>Nawaikoke Sub-county</rdfs:label>
    </owl:NamedIndividual>
    


    <!-- http://purl.obolibrary.org/obo/GAZ_00236741 -->

    <owl:NamedIndividual rdf:about="http://purl.obolibrary.org/obo/GAZ_00236741">
        <obo:RO_0001025 rdf:resource="http://purl.obolibrary.org/obo/GAZ_00015470"/>
        <obo:IAO_0000115>A fourth-level administrative division of Uganda.</obo:IAO_0000115>
        <oboInOwl:hasOBONamespace>GAZ</oboInOwl:hasOBONamespace>
        <oboInOwl:id>GAZ:00236741</oboInOwl:id>
        <rdfs:label>Kaliro Town</rdfs:label>
    </owl:NamedIndividual>
    


    <!-- http://purl.obolibrary.org/obo/GAZ_00236742 -->

    <owl:NamedIndividual rdf:about="http://purl.obolibrary.org/obo/GAZ_00236742">
        <obo:RO_0001025 rdf:resource="http://purl.obolibrary.org/obo/GAZ_00015471"/>
        <obo:IAO_0000115>A fourth-level administrative division of Uganda.</obo:IAO_0000115>
        <oboInOwl:hasOBONamespace>GAZ</oboInOwl:hasOBONamespace>
        <oboInOwl:id>GAZ:00236742</oboInOwl:id>
        <rdfs:label>Bugaya Sub-county</rdfs:label>
    </owl:NamedIndividual>
    


    <!-- http://purl.obolibrary.org/obo/GAZ_00236743 -->

    <owl:NamedIndividual rdf:about="http://purl.obolibrary.org/obo/GAZ_00236743">
        <obo:RO_0001025 rdf:resource="http://purl.obolibrary.org/obo/GAZ_00015471"/>
        <obo:IAO_0000115>A fourth-level administrative division of Uganda.</obo:IAO_0000115>
        <oboInOwl:hasOBONamespace>GAZ</oboInOwl:hasOBONamespace>
        <oboInOwl:id>GAZ:00236743</oboInOwl:id>
        <rdfs:label>Buyende Sub-county</rdfs:label>
    </owl:NamedIndividual>
    


    <!-- http://purl.obolibrary.org/obo/GAZ_00236744 -->

    <owl:NamedIndividual rdf:about="http://purl.obolibrary.org/obo/GAZ_00236744">
        <obo:RO_0001025 rdf:resource="http://purl.obolibrary.org/obo/GAZ_00015471"/>
        <obo:IAO_0000115>A fourth-level administrative division of Uganda.</obo:IAO_0000115>
        <oboInOwl:hasOBONamespace>GAZ</oboInOwl:hasOBONamespace>
        <oboInOwl:id>GAZ:00236744</oboInOwl:id>
        <rdfs:label>Kagulu Sub-county</rdfs:label>
    </owl:NamedIndividual>
    


    <!-- http://purl.obolibrary.org/obo/GAZ_00236745 -->

    <owl:NamedIndividual rdf:about="http://purl.obolibrary.org/obo/GAZ_00236745">
        <obo:RO_0001025 rdf:resource="http://purl.obolibrary.org/obo/GAZ_00015471"/>
        <obo:IAO_0000115>A fourth-level administrative division of Uganda.</obo:IAO_0000115>
        <oboInOwl:hasOBONamespace>GAZ</oboInOwl:hasOBONamespace>
        <oboInOwl:id>GAZ:00236745</oboInOwl:id>
        <rdfs:label>Kidera Sub-county</rdfs:label>
    </owl:NamedIndividual>
    


    <!-- http://purl.obolibrary.org/obo/GAZ_00236746 -->

    <owl:NamedIndividual rdf:about="http://purl.obolibrary.org/obo/GAZ_00236746">
        <obo:RO_0001025 rdf:resource="http://purl.obolibrary.org/obo/GAZ_00015471"/>
        <obo:IAO_0000115>A fourth-level administrative division of Uganda.</obo:IAO_0000115>
        <oboInOwl:hasOBONamespace>GAZ</oboInOwl:hasOBONamespace>
        <oboInOwl:id>GAZ:00236746</oboInOwl:id>
        <rdfs:label>Nkondo Sub-county</rdfs:label>
    </owl:NamedIndividual>
    


    <!-- http://purl.obolibrary.org/obo/GAZ_00236747 -->

    <owl:NamedIndividual rdf:about="http://purl.obolibrary.org/obo/GAZ_00236747">
        <obo:RO_0001025 rdf:resource="http://purl.obolibrary.org/obo/GAZ_00015472"/>
        <obo:IAO_0000115>A fourth-level administrative division of Uganda.</obo:IAO_0000115>
        <oboInOwl:hasOBONamespace>GAZ</oboInOwl:hasOBONamespace>
        <oboInOwl:id>GAZ:00236747</oboInOwl:id>
        <rdfs:label>Balawoli Sub-county</rdfs:label>
    </owl:NamedIndividual>
    


    <!-- http://purl.obolibrary.org/obo/GAZ_00236748 -->

    <owl:NamedIndividual rdf:about="http://purl.obolibrary.org/obo/GAZ_00236748">
        <obo:RO_0001025 rdf:resource="http://purl.obolibrary.org/obo/GAZ_00015472"/>
        <obo:IAO_0000115>A fourth-level administrative division of Uganda.</obo:IAO_0000115>
        <oboInOwl:hasOBONamespace>GAZ</oboInOwl:hasOBONamespace>
        <oboInOwl:id>GAZ:00236748</oboInOwl:id>
        <rdfs:label>Bulopa Sub-county</rdfs:label>
    </owl:NamedIndividual>
    


    <!-- http://purl.obolibrary.org/obo/GAZ_00236749 -->

    <owl:NamedIndividual rdf:about="http://purl.obolibrary.org/obo/GAZ_00236749">
        <obo:RO_0001025 rdf:resource="http://purl.obolibrary.org/obo/GAZ_00015472"/>
        <obo:IAO_0000115>A fourth-level administrative division of Uganda.</obo:IAO_0000115>
        <oboInOwl:hasOBONamespace>GAZ</oboInOwl:hasOBONamespace>
        <oboInOwl:id>GAZ:00236749</oboInOwl:id>
        <rdfs:label>Butansi Sub-county</rdfs:label>
    </owl:NamedIndividual>
    


    <!-- http://purl.obolibrary.org/obo/GAZ_00236750 -->

    <owl:NamedIndividual rdf:about="http://purl.obolibrary.org/obo/GAZ_00236750">
        <obo:RO_0001025 rdf:resource="http://purl.obolibrary.org/obo/GAZ_00015472"/>
        <obo:IAO_0000115>A fourth-level administrative division of Uganda.</obo:IAO_0000115>
        <oboInOwl:hasOBONamespace>GAZ</oboInOwl:hasOBONamespace>
        <oboInOwl:id>GAZ:00236750</oboInOwl:id>
        <rdfs:label>Kamuli Town</rdfs:label>
    </owl:NamedIndividual>
    


    <!-- http://purl.obolibrary.org/obo/GAZ_00236751 -->

    <owl:NamedIndividual rdf:about="http://purl.obolibrary.org/obo/GAZ_00236751">
        <obo:RO_0001025 rdf:resource="http://purl.obolibrary.org/obo/GAZ_00015472"/>
        <obo:IAO_0000115>A fourth-level administrative division of Uganda.</obo:IAO_0000115>
        <oboInOwl:hasOBONamespace>GAZ</oboInOwl:hasOBONamespace>
        <oboInOwl:id>GAZ:00236751</oboInOwl:id>
        <rdfs:label>Kitayunjwa Sub-county</rdfs:label>
    </owl:NamedIndividual>
    


    <!-- http://purl.obolibrary.org/obo/GAZ_00236752 -->

    <owl:NamedIndividual rdf:about="http://purl.obolibrary.org/obo/GAZ_00236752">
        <obo:RO_0001025 rdf:resource="http://purl.obolibrary.org/obo/GAZ_00015472"/>
        <obo:IAO_0000115>A fourth-level administrative division of Uganda.</obo:IAO_0000115>
        <oboInOwl:hasOBONamespace>GAZ</oboInOwl:hasOBONamespace>
        <oboInOwl:id>GAZ:00236752</oboInOwl:id>
        <rdfs:label>Nabwigulu Sub-county</rdfs:label>
    </owl:NamedIndividual>
    


    <!-- http://purl.obolibrary.org/obo/GAZ_00236753 -->

    <owl:NamedIndividual rdf:about="http://purl.obolibrary.org/obo/GAZ_00236753">
        <obo:RO_0001025 rdf:resource="http://purl.obolibrary.org/obo/GAZ_00015472"/>
        <obo:IAO_0000115>A fourth-level administrative division of Uganda.</obo:IAO_0000115>
        <oboInOwl:hasOBONamespace>GAZ</oboInOwl:hasOBONamespace>
        <oboInOwl:id>GAZ:00236753</oboInOwl:id>
        <rdfs:label>Namasagali Sub-county</rdfs:label>
    </owl:NamedIndividual>
    


    <!-- http://purl.obolibrary.org/obo/GAZ_00236754 -->

    <owl:NamedIndividual rdf:about="http://purl.obolibrary.org/obo/GAZ_00236754">
        <obo:RO_0001025 rdf:resource="http://purl.obolibrary.org/obo/GAZ_00015472"/>
        <obo:IAO_0000115>A fourth-level administrative division of Uganda.</obo:IAO_0000115>
        <oboInOwl:hasOBONamespace>GAZ</oboInOwl:hasOBONamespace>
        <oboInOwl:id>GAZ:00236754</oboInOwl:id>
        <rdfs:label>Namwendwa Sub-county</rdfs:label>
    </owl:NamedIndividual>
    


    <!-- http://purl.obolibrary.org/obo/GAZ_00236755 -->

    <owl:NamedIndividual rdf:about="http://purl.obolibrary.org/obo/GAZ_00236755">
        <obo:RO_0001025 rdf:resource="http://purl.obolibrary.org/obo/GAZ_00015473"/>
        <obo:IAO_0000115>A fourth-level administrative division of Uganda.</obo:IAO_0000115>
        <oboInOwl:hasOBONamespace>GAZ</oboInOwl:hasOBONamespace>
        <oboInOwl:id>GAZ:00236755</oboInOwl:id>
        <rdfs:label>Bugulumbya Sub-county</rdfs:label>
    </owl:NamedIndividual>
    


    <!-- http://purl.obolibrary.org/obo/GAZ_00236756 -->

    <owl:NamedIndividual rdf:about="http://purl.obolibrary.org/obo/GAZ_00236756">
        <obo:RO_0001025 rdf:resource="http://purl.obolibrary.org/obo/GAZ_00015473"/>
        <obo:IAO_0000115>A fourth-level administrative division of Uganda.</obo:IAO_0000115>
        <oboInOwl:hasOBONamespace>GAZ</oboInOwl:hasOBONamespace>
        <oboInOwl:id>GAZ:00236756</oboInOwl:id>
        <rdfs:label>Kisozi Sub-county</rdfs:label>
    </owl:NamedIndividual>
    


    <!-- http://purl.obolibrary.org/obo/GAZ_00236757 -->

    <owl:NamedIndividual rdf:about="http://purl.obolibrary.org/obo/GAZ_00236757">
        <obo:RO_0001025 rdf:resource="http://purl.obolibrary.org/obo/GAZ_00015473"/>
        <obo:IAO_0000115>A fourth-level administrative division of Uganda.</obo:IAO_0000115>
        <oboInOwl:hasOBONamespace>GAZ</oboInOwl:hasOBONamespace>
        <oboInOwl:id>GAZ:00236757</oboInOwl:id>
        <rdfs:label>Mbulamuti Sub-county</rdfs:label>
    </owl:NamedIndividual>
    


    <!-- http://purl.obolibrary.org/obo/GAZ_00236758 -->

    <owl:NamedIndividual rdf:about="http://purl.obolibrary.org/obo/GAZ_00236758">
        <obo:RO_0001025 rdf:resource="http://purl.obolibrary.org/obo/GAZ_00015473"/>
        <obo:IAO_0000115>A fourth-level administrative division of Uganda.</obo:IAO_0000115>
        <oboInOwl:hasOBONamespace>GAZ</oboInOwl:hasOBONamespace>
        <oboInOwl:id>GAZ:00236758</oboInOwl:id>
        <rdfs:label>Nawanyago Sub-county</rdfs:label>
    </owl:NamedIndividual>
    


    <!-- http://purl.obolibrary.org/obo/GAZ_00236759 -->

    <owl:NamedIndividual rdf:about="http://purl.obolibrary.org/obo/GAZ_00236759">
        <obo:RO_0001025 rdf:resource="http://purl.obolibrary.org/obo/GAZ_00015473"/>
        <obo:IAO_0000115>A fourth-level administrative division of Uganda.</obo:IAO_0000115>
        <oboInOwl:hasOBONamespace>GAZ</oboInOwl:hasOBONamespace>
        <oboInOwl:id>GAZ:00236759</oboInOwl:id>
        <rdfs:label>Wankole Sub-county</rdfs:label>
    </owl:NamedIndividual>
    


    <!-- http://purl.obolibrary.org/obo/GAZ_00236760 -->

    <owl:NamedIndividual rdf:about="http://purl.obolibrary.org/obo/GAZ_00236760">
        <obo:RO_0001025 rdf:resource="http://purl.obolibrary.org/obo/GAZ_00015474"/>
        <obo:IAO_0000115>A fourth-level administrative division of Uganda.</obo:IAO_0000115>
        <oboInOwl:hasOBONamespace>GAZ</oboInOwl:hasOBONamespace>
        <oboInOwl:id>GAZ:00236760</oboInOwl:id>
        <rdfs:label>Benet Sub-county</rdfs:label>
    </owl:NamedIndividual>
    


    <!-- http://purl.obolibrary.org/obo/GAZ_00236761 -->

    <owl:NamedIndividual rdf:about="http://purl.obolibrary.org/obo/GAZ_00236761">
        <obo:RO_0001025 rdf:resource="http://purl.obolibrary.org/obo/GAZ_00015474"/>
        <obo:IAO_0000115>A fourth-level administrative division of Uganda.</obo:IAO_0000115>
        <oboInOwl:hasOBONamespace>GAZ</oboInOwl:hasOBONamespace>
        <oboInOwl:id>GAZ:00236761</oboInOwl:id>
        <rdfs:label>Binyiny Sub-county</rdfs:label>
    </owl:NamedIndividual>
    


    <!-- http://purl.obolibrary.org/obo/GAZ_00236762 -->

    <owl:NamedIndividual rdf:about="http://purl.obolibrary.org/obo/GAZ_00236762">
        <obo:RO_0001025 rdf:resource="http://purl.obolibrary.org/obo/GAZ_00015474"/>
        <obo:IAO_0000115>A fourth-level administrative division of Uganda.</obo:IAO_0000115>
        <oboInOwl:hasOBONamespace>GAZ</oboInOwl:hasOBONamespace>
        <oboInOwl:id>GAZ:00236762</oboInOwl:id>
        <rdfs:label>Kaproron Sub-county</rdfs:label>
    </owl:NamedIndividual>
    


    <!-- http://purl.obolibrary.org/obo/GAZ_00236763 -->

    <owl:NamedIndividual rdf:about="http://purl.obolibrary.org/obo/GAZ_00236763">
        <obo:RO_0001025 rdf:resource="http://purl.obolibrary.org/obo/GAZ_00015474"/>
        <obo:IAO_0000115>A fourth-level administrative division of Uganda.</obo:IAO_0000115>
        <oboInOwl:hasOBONamespace>GAZ</oboInOwl:hasOBONamespace>
        <oboInOwl:id>GAZ:00236763</oboInOwl:id>
        <rdfs:label>Kwanyiny Sub-county</rdfs:label>
    </owl:NamedIndividual>
    


    <!-- http://purl.obolibrary.org/obo/GAZ_00236764 -->

    <owl:NamedIndividual rdf:about="http://purl.obolibrary.org/obo/GAZ_00236764">
        <obo:RO_0001025 rdf:resource="http://purl.obolibrary.org/obo/GAZ_00015474"/>
        <obo:IAO_0000115>A fourth-level administrative division of Uganda.</obo:IAO_0000115>
        <oboInOwl:hasOBONamespace>GAZ</oboInOwl:hasOBONamespace>
        <oboInOwl:id>GAZ:00236764</oboInOwl:id>
        <rdfs:label>Ngenge Sub-county</rdfs:label>
    </owl:NamedIndividual>
    


    <!-- http://purl.obolibrary.org/obo/GAZ_00236765 -->

    <owl:NamedIndividual rdf:about="http://purl.obolibrary.org/obo/GAZ_00236765">
        <obo:RO_0001025 rdf:resource="http://purl.obolibrary.org/obo/GAZ_00015475"/>
        <obo:IAO_0000115>A fourth-level administrative division of Uganda.</obo:IAO_0000115>
        <oboInOwl:hasOBONamespace>GAZ</oboInOwl:hasOBONamespace>
        <oboInOwl:id>GAZ:00236765</oboInOwl:id>
        <rdfs:label>Chema Sub-county</rdfs:label>
    </owl:NamedIndividual>
    


    <!-- http://purl.obolibrary.org/obo/GAZ_00236766 -->

    <owl:NamedIndividual rdf:about="http://purl.obolibrary.org/obo/GAZ_00236766">
        <obo:RO_0001025 rdf:resource="http://purl.obolibrary.org/obo/GAZ_00015475"/>
        <obo:IAO_0000115>A fourth-level administrative division of Uganda.</obo:IAO_0000115>
        <oboInOwl:hasOBONamespace>GAZ</oboInOwl:hasOBONamespace>
        <oboInOwl:id>GAZ:00236766</oboInOwl:id>
        <rdfs:label>Kapchorwa Town</rdfs:label>
    </owl:NamedIndividual>
    


    <!-- http://purl.obolibrary.org/obo/GAZ_00236767 -->

    <owl:NamedIndividual rdf:about="http://purl.obolibrary.org/obo/GAZ_00236767">
        <obo:RO_0001025 rdf:resource="http://purl.obolibrary.org/obo/GAZ_00015475"/>
        <obo:IAO_0000115>A fourth-level administrative division of Uganda.</obo:IAO_0000115>
        <oboInOwl:hasOBONamespace>GAZ</oboInOwl:hasOBONamespace>
        <oboInOwl:id>GAZ:00236767</oboInOwl:id>
        <rdfs:label>Kaptanya Sub-county</rdfs:label>
    </owl:NamedIndividual>
    


    <!-- http://purl.obolibrary.org/obo/GAZ_00236768 -->

    <owl:NamedIndividual rdf:about="http://purl.obolibrary.org/obo/GAZ_00236768">
        <obo:RO_0001025 rdf:resource="http://purl.obolibrary.org/obo/GAZ_00015475"/>
        <obo:IAO_0000115>A fourth-level administrative division of Uganda.</obo:IAO_0000115>
        <oboInOwl:hasOBONamespace>GAZ</oboInOwl:hasOBONamespace>
        <oboInOwl:id>GAZ:00236768</oboInOwl:id>
        <rdfs:label>Kaserem Sub-county</rdfs:label>
    </owl:NamedIndividual>
    


    <!-- http://purl.obolibrary.org/obo/GAZ_00236769 -->

    <owl:NamedIndividual rdf:about="http://purl.obolibrary.org/obo/GAZ_00236769">
        <obo:RO_0001025 rdf:resource="http://purl.obolibrary.org/obo/GAZ_00015475"/>
        <obo:IAO_0000115>A fourth-level administrative division of Uganda.</obo:IAO_0000115>
        <oboInOwl:hasOBONamespace>GAZ</oboInOwl:hasOBONamespace>
        <oboInOwl:id>GAZ:00236769</oboInOwl:id>
        <rdfs:label>Kawowo Sub-county</rdfs:label>
    </owl:NamedIndividual>
    


    <!-- http://purl.obolibrary.org/obo/GAZ_00236770 -->

    <owl:NamedIndividual rdf:about="http://purl.obolibrary.org/obo/GAZ_00236770">
        <obo:RO_0001025 rdf:resource="http://purl.obolibrary.org/obo/GAZ_00015475"/>
        <obo:IAO_0000115>A fourth-level administrative division of Uganda.</obo:IAO_0000115>
        <oboInOwl:hasOBONamespace>GAZ</oboInOwl:hasOBONamespace>
        <oboInOwl:id>GAZ:00236770</oboInOwl:id>
        <rdfs:label>Sipi Sub-county</rdfs:label>
    </owl:NamedIndividual>
    


    <!-- http://purl.obolibrary.org/obo/GAZ_00236771 -->

    <owl:NamedIndividual rdf:about="http://purl.obolibrary.org/obo/GAZ_00236771">
        <obo:RO_0001025 rdf:resource="http://purl.obolibrary.org/obo/GAZ_00015475"/>
        <obo:IAO_0000115>A fourth-level administrative division of Uganda.</obo:IAO_0000115>
        <oboInOwl:hasOBONamespace>GAZ</oboInOwl:hasOBONamespace>
        <oboInOwl:id>GAZ:00236771</oboInOwl:id>
        <rdfs:label>Tegeres Sub-county</rdfs:label>
    </owl:NamedIndividual>
    


    <!-- http://purl.obolibrary.org/obo/GAZ_00236772 -->

    <owl:NamedIndividual rdf:about="http://purl.obolibrary.org/obo/GAZ_00236772">
        <obo:RO_0001025 rdf:resource="http://purl.obolibrary.org/obo/GAZ_00015477"/>
        <obo:IAO_0000115>A fourth-level administrative division of Uganda.</obo:IAO_0000115>
        <oboInOwl:hasOBONamespace>GAZ</oboInOwl:hasOBONamespace>
        <oboInOwl:id>GAZ:00236772</oboInOwl:id>
        <rdfs:label>Atutur Sub-county</rdfs:label>
    </owl:NamedIndividual>
    


    <!-- http://purl.obolibrary.org/obo/GAZ_00236773 -->

    <owl:NamedIndividual rdf:about="http://purl.obolibrary.org/obo/GAZ_00236773">
        <obo:RO_0001025 rdf:resource="http://purl.obolibrary.org/obo/GAZ_00015477"/>
        <obo:IAO_0000115>A fourth-level administrative division of Uganda.</obo:IAO_0000115>
        <oboInOwl:hasOBONamespace>GAZ</oboInOwl:hasOBONamespace>
        <oboInOwl:id>GAZ:00236773</oboInOwl:id>
        <rdfs:label>Kanyum Sub-county</rdfs:label>
    </owl:NamedIndividual>
    


    <!-- http://purl.obolibrary.org/obo/GAZ_00236774 -->

    <owl:NamedIndividual rdf:about="http://purl.obolibrary.org/obo/GAZ_00236774">
        <obo:RO_0001025 rdf:resource="http://purl.obolibrary.org/obo/GAZ_00015477"/>
        <obo:IAO_0000115>A fourth-level administrative division of Uganda.</obo:IAO_0000115>
        <oboInOwl:hasOBONamespace>GAZ</oboInOwl:hasOBONamespace>
        <oboInOwl:id>GAZ:00236774</oboInOwl:id>
        <rdfs:label>Kumi Sub-county</rdfs:label>
    </owl:NamedIndividual>
    


    <!-- http://purl.obolibrary.org/obo/GAZ_00236775 -->

    <owl:NamedIndividual rdf:about="http://purl.obolibrary.org/obo/GAZ_00236775">
        <obo:RO_0001025 rdf:resource="http://purl.obolibrary.org/obo/GAZ_00015477"/>
        <obo:IAO_0000115>A fourth-level administrative division of Uganda.</obo:IAO_0000115>
        <oboInOwl:hasOBONamespace>GAZ</oboInOwl:hasOBONamespace>
        <oboInOwl:id>GAZ:00236775</oboInOwl:id>
        <rdfs:label>Kumi Town</rdfs:label>
    </owl:NamedIndividual>
    


    <!-- http://purl.obolibrary.org/obo/GAZ_00236776 -->

    <owl:NamedIndividual rdf:about="http://purl.obolibrary.org/obo/GAZ_00236776">
        <obo:RO_0001025 rdf:resource="http://purl.obolibrary.org/obo/GAZ_00015477"/>
        <obo:IAO_0000115>A fourth-level administrative division of Uganda.</obo:IAO_0000115>
        <oboInOwl:hasOBONamespace>GAZ</oboInOwl:hasOBONamespace>
        <oboInOwl:id>GAZ:00236776</oboInOwl:id>
        <rdfs:label>Mukongoro Sub-county</rdfs:label>
    </owl:NamedIndividual>
    


    <!-- http://purl.obolibrary.org/obo/GAZ_00236777 -->

    <owl:NamedIndividual rdf:about="http://purl.obolibrary.org/obo/GAZ_00236777">
        <obo:RO_0001025 rdf:resource="http://purl.obolibrary.org/obo/GAZ_00015477"/>
        <obo:IAO_0000115>A fourth-level administrative division of Uganda.</obo:IAO_0000115>
        <oboInOwl:hasOBONamespace>GAZ</oboInOwl:hasOBONamespace>
        <oboInOwl:id>GAZ:00236777</oboInOwl:id>
        <rdfs:label>Nyero Sub-county</rdfs:label>
    </owl:NamedIndividual>
    


    <!-- http://purl.obolibrary.org/obo/GAZ_00236778 -->

    <owl:NamedIndividual rdf:about="http://purl.obolibrary.org/obo/GAZ_00236778">
        <obo:RO_0001025 rdf:resource="http://purl.obolibrary.org/obo/GAZ_00015477"/>
        <obo:IAO_0000115>A fourth-level administrative division of Uganda.</obo:IAO_0000115>
        <oboInOwl:hasOBONamespace>GAZ</oboInOwl:hasOBONamespace>
        <oboInOwl:id>GAZ:00236778</oboInOwl:id>
        <rdfs:label>Ongino Sub-county</rdfs:label>
    </owl:NamedIndividual>
    


    <!-- http://purl.obolibrary.org/obo/GAZ_00236779 -->

    <owl:NamedIndividual rdf:about="http://purl.obolibrary.org/obo/GAZ_00236779">
        <obo:RO_0001025 rdf:resource="http://purl.obolibrary.org/obo/GAZ_00015478"/>
        <obo:IAO_0000115>A fourth-level administrative division of Uganda.</obo:IAO_0000115>
        <oboInOwl:hasOBONamespace>GAZ</oboInOwl:hasOBONamespace>
        <oboInOwl:id>GAZ:00236779</oboInOwl:id>
        <rdfs:label>Kapir Sub-county</rdfs:label>
    </owl:NamedIndividual>
    


    <!-- http://purl.obolibrary.org/obo/GAZ_00236780 -->

    <owl:NamedIndividual rdf:about="http://purl.obolibrary.org/obo/GAZ_00236780">
        <obo:RO_0001025 rdf:resource="http://purl.obolibrary.org/obo/GAZ_00015478"/>
        <obo:IAO_0000115>A fourth-level administrative division of Uganda.</obo:IAO_0000115>
        <oboInOwl:hasOBONamespace>GAZ</oboInOwl:hasOBONamespace>
        <oboInOwl:id>GAZ:00236780</oboInOwl:id>
        <rdfs:label>Kobwin Sub-county</rdfs:label>
    </owl:NamedIndividual>
    


    <!-- http://purl.obolibrary.org/obo/GAZ_00236781 -->

    <owl:NamedIndividual rdf:about="http://purl.obolibrary.org/obo/GAZ_00236781">
        <obo:RO_0001025 rdf:resource="http://purl.obolibrary.org/obo/GAZ_00015478"/>
        <obo:IAO_0000115>A fourth-level administrative division of Uganda.</obo:IAO_0000115>
        <oboInOwl:hasOBONamespace>GAZ</oboInOwl:hasOBONamespace>
        <oboInOwl:id>GAZ:00236781</oboInOwl:id>
        <rdfs:label>Mukura Sub-county</rdfs:label>
    </owl:NamedIndividual>
    


    <!-- http://purl.obolibrary.org/obo/GAZ_00236782 -->

    <owl:NamedIndividual rdf:about="http://purl.obolibrary.org/obo/GAZ_00236782">
        <obo:RO_0001025 rdf:resource="http://purl.obolibrary.org/obo/GAZ_00015478"/>
        <obo:IAO_0000115>A fourth-level administrative division of Uganda.</obo:IAO_0000115>
        <oboInOwl:hasOBONamespace>GAZ</oboInOwl:hasOBONamespace>
        <oboInOwl:id>GAZ:00236782</oboInOwl:id>
        <rdfs:label>Ngora Sub-county</rdfs:label>
    </owl:NamedIndividual>
    


    <!-- http://purl.obolibrary.org/obo/GAZ_00236783 -->

    <owl:NamedIndividual rdf:about="http://purl.obolibrary.org/obo/GAZ_00236783">
        <obo:RO_0001025 rdf:resource="http://purl.obolibrary.org/obo/GAZ_00015479"/>
        <obo:IAO_0000115>A fourth-level administrative division of Uganda.</obo:IAO_0000115>
        <oboInOwl:hasOBONamespace>GAZ</oboInOwl:hasOBONamespace>
        <oboInOwl:id>GAZ:00236783</oboInOwl:id>
        <rdfs:label>Bubutu Sub-county</rdfs:label>
    </owl:NamedIndividual>
    


    <!-- http://purl.obolibrary.org/obo/GAZ_00236784 -->

    <owl:NamedIndividual rdf:about="http://purl.obolibrary.org/obo/GAZ_00236784">
        <obo:RO_0001025 rdf:resource="http://purl.obolibrary.org/obo/GAZ_00015479"/>
        <obo:IAO_0000115>A fourth-level administrative division of Uganda.</obo:IAO_0000115>
        <oboInOwl:hasOBONamespace>GAZ</oboInOwl:hasOBONamespace>
        <oboInOwl:id>GAZ:00236784</oboInOwl:id>
        <rdfs:label>Bugobero Sub-county</rdfs:label>
    </owl:NamedIndividual>
    


    <!-- http://purl.obolibrary.org/obo/GAZ_00236785 -->

    <owl:NamedIndividual rdf:about="http://purl.obolibrary.org/obo/GAZ_00236785">
        <obo:RO_0001025 rdf:resource="http://purl.obolibrary.org/obo/GAZ_00015479"/>
        <obo:IAO_0000115>A fourth-level administrative division of Uganda.</obo:IAO_0000115>
        <oboInOwl:hasOBONamespace>GAZ</oboInOwl:hasOBONamespace>
        <oboInOwl:id>GAZ:00236785</oboInOwl:id>
        <rdfs:label>Bumbo Sub-county</rdfs:label>
    </owl:NamedIndividual>
    


    <!-- http://purl.obolibrary.org/obo/GAZ_00236786 -->

    <owl:NamedIndividual rdf:about="http://purl.obolibrary.org/obo/GAZ_00236786">
        <obo:RO_0001025 rdf:resource="http://purl.obolibrary.org/obo/GAZ_00015479"/>
        <obo:IAO_0000115>A fourth-level administrative division of Uganda.</obo:IAO_0000115>
        <oboInOwl:hasOBONamespace>GAZ</oboInOwl:hasOBONamespace>
        <oboInOwl:id>GAZ:00236786</oboInOwl:id>
        <rdfs:label>Bumwoni Sub-county</rdfs:label>
    </owl:NamedIndividual>
    


    <!-- http://purl.obolibrary.org/obo/GAZ_00236787 -->

    <owl:NamedIndividual rdf:about="http://purl.obolibrary.org/obo/GAZ_00236787">
        <obo:RO_0001025 rdf:resource="http://purl.obolibrary.org/obo/GAZ_00015479"/>
        <obo:IAO_0000115>A fourth-level administrative division of Uganda.</obo:IAO_0000115>
        <oboInOwl:hasOBONamespace>GAZ</oboInOwl:hasOBONamespace>
        <oboInOwl:id>GAZ:00236787</oboInOwl:id>
        <rdfs:label>Bupoto Sub-county</rdfs:label>
    </owl:NamedIndividual>
    


    <!-- http://purl.obolibrary.org/obo/GAZ_00236788 -->

    <owl:NamedIndividual rdf:about="http://purl.obolibrary.org/obo/GAZ_00236788">
        <obo:RO_0001025 rdf:resource="http://purl.obolibrary.org/obo/GAZ_00015479"/>
        <obo:IAO_0000115>A fourth-level administrative division of Uganda.</obo:IAO_0000115>
        <oboInOwl:hasOBONamespace>GAZ</oboInOwl:hasOBONamespace>
        <oboInOwl:id>GAZ:00236788</oboInOwl:id>
        <rdfs:label>Butiru Sub-county</rdfs:label>
    </owl:NamedIndividual>
    


    <!-- http://purl.obolibrary.org/obo/GAZ_00236789 -->

    <owl:NamedIndividual rdf:about="http://purl.obolibrary.org/obo/GAZ_00236789">
        <obo:RO_0001025 rdf:resource="http://purl.obolibrary.org/obo/GAZ_00015479"/>
        <obo:IAO_0000115>A fourth-level administrative division of Uganda.</obo:IAO_0000115>
        <oboInOwl:hasOBONamespace>GAZ</oboInOwl:hasOBONamespace>
        <oboInOwl:id>GAZ:00236789</oboInOwl:id>
        <rdfs:label>Buwabwala Sub-county</rdfs:label>
    </owl:NamedIndividual>
    


    <!-- http://purl.obolibrary.org/obo/GAZ_00236790 -->

    <owl:NamedIndividual rdf:about="http://purl.obolibrary.org/obo/GAZ_00236790">
        <obo:RO_0001025 rdf:resource="http://purl.obolibrary.org/obo/GAZ_00015479"/>
        <obo:IAO_0000115>A fourth-level administrative division of Uganda.</obo:IAO_0000115>
        <oboInOwl:hasOBONamespace>GAZ</oboInOwl:hasOBONamespace>
        <oboInOwl:id>GAZ:00236790</oboInOwl:id>
        <rdfs:label>Buwagogo Sub-county</rdfs:label>
    </owl:NamedIndividual>
    


    <!-- http://purl.obolibrary.org/obo/GAZ_00236791 -->

    <owl:NamedIndividual rdf:about="http://purl.obolibrary.org/obo/GAZ_00236791">
        <obo:RO_0001025 rdf:resource="http://purl.obolibrary.org/obo/GAZ_00015479"/>
        <obo:IAO_0000115>A fourth-level administrative division of Uganda.</obo:IAO_0000115>
        <oboInOwl:hasOBONamespace>GAZ</oboInOwl:hasOBONamespace>
        <oboInOwl:id>GAZ:00236791</oboInOwl:id>
        <rdfs:label>Kaato Sub-county</rdfs:label>
    </owl:NamedIndividual>
    


    <!-- http://purl.obolibrary.org/obo/GAZ_00236792 -->

    <owl:NamedIndividual rdf:about="http://purl.obolibrary.org/obo/GAZ_00236792">
        <obo:RO_0001025 rdf:resource="http://purl.obolibrary.org/obo/GAZ_00015479"/>
        <obo:IAO_0000115>A fourth-level administrative division of Uganda.</obo:IAO_0000115>
        <oboInOwl:hasOBONamespace>GAZ</oboInOwl:hasOBONamespace>
        <oboInOwl:id>GAZ:00236792</oboInOwl:id>
        <rdfs:label>Sibanga Sub-county</rdfs:label>
    </owl:NamedIndividual>
    


    <!-- http://purl.obolibrary.org/obo/GAZ_00236793 -->

    <owl:NamedIndividual rdf:about="http://purl.obolibrary.org/obo/GAZ_00236793">
        <obo:RO_0001025 rdf:resource="http://purl.obolibrary.org/obo/GAZ_00015480"/>
        <obo:IAO_0000115>A fourth-level administrative division of Uganda.</obo:IAO_0000115>
        <oboInOwl:hasOBONamespace>GAZ</oboInOwl:hasOBONamespace>
        <oboInOwl:id>GAZ:00236793</oboInOwl:id>
        <rdfs:label>Bubiita Sub-county</rdfs:label>
    </owl:NamedIndividual>
    


    <!-- http://purl.obolibrary.org/obo/GAZ_00236794 -->

    <owl:NamedIndividual rdf:about="http://purl.obolibrary.org/obo/GAZ_00236794">
        <obo:RO_0001025 rdf:resource="http://purl.obolibrary.org/obo/GAZ_00015480"/>
        <obo:IAO_0000115>A fourth-level administrative division of Uganda.</obo:IAO_0000115>
        <oboInOwl:hasOBONamespace>GAZ</oboInOwl:hasOBONamespace>
        <oboInOwl:id>GAZ:00236794</oboInOwl:id>
        <rdfs:label>Bududa Sub-county</rdfs:label>
    </owl:NamedIndividual>
    


    <!-- http://purl.obolibrary.org/obo/GAZ_00236795 -->

    <owl:NamedIndividual rdf:about="http://purl.obolibrary.org/obo/GAZ_00236795">
        <obo:RO_0001025 rdf:resource="http://purl.obolibrary.org/obo/GAZ_00015480"/>
        <obo:IAO_0000115>A fourth-level administrative division of Uganda.</obo:IAO_0000115>
        <oboInOwl:hasOBONamespace>GAZ</oboInOwl:hasOBONamespace>
        <oboInOwl:id>GAZ:00236795</oboInOwl:id>
        <rdfs:label>Bukibokolo Sub-county</rdfs:label>
    </owl:NamedIndividual>
    


    <!-- http://purl.obolibrary.org/obo/GAZ_00236796 -->

    <owl:NamedIndividual rdf:about="http://purl.obolibrary.org/obo/GAZ_00236796">
        <obo:RO_0001025 rdf:resource="http://purl.obolibrary.org/obo/GAZ_00015480"/>
        <obo:IAO_0000115>A fourth-level administrative division of Uganda.</obo:IAO_0000115>
        <oboInOwl:hasOBONamespace>GAZ</oboInOwl:hasOBONamespace>
        <oboInOwl:id>GAZ:00236796</oboInOwl:id>
        <rdfs:label>Bukigai Sub-county</rdfs:label>
    </owl:NamedIndividual>
    


    <!-- http://purl.obolibrary.org/obo/GAZ_00236797 -->

    <owl:NamedIndividual rdf:about="http://purl.obolibrary.org/obo/GAZ_00236797">
        <obo:RO_0001025 rdf:resource="http://purl.obolibrary.org/obo/GAZ_00015480"/>
        <obo:IAO_0000115>A fourth-level administrative division of Uganda.</obo:IAO_0000115>
        <oboInOwl:hasOBONamespace>GAZ</oboInOwl:hasOBONamespace>
        <oboInOwl:id>GAZ:00236797</oboInOwl:id>
        <rdfs:label>Bulucheke Sub-county</rdfs:label>
    </owl:NamedIndividual>
    


    <!-- http://purl.obolibrary.org/obo/GAZ_00236798 -->

    <owl:NamedIndividual rdf:about="http://purl.obolibrary.org/obo/GAZ_00236798">
        <obo:RO_0001025 rdf:resource="http://purl.obolibrary.org/obo/GAZ_00015480"/>
        <obo:IAO_0000115>A fourth-level administrative division of Uganda.</obo:IAO_0000115>
        <oboInOwl:hasOBONamespace>GAZ</oboInOwl:hasOBONamespace>
        <oboInOwl:id>GAZ:00236798</oboInOwl:id>
        <rdfs:label>Bumayoka Sub-county</rdfs:label>
    </owl:NamedIndividual>
    


    <!-- http://purl.obolibrary.org/obo/GAZ_00236799 -->

    <owl:NamedIndividual rdf:about="http://purl.obolibrary.org/obo/GAZ_00236799">
        <obo:RO_0001025 rdf:resource="http://purl.obolibrary.org/obo/GAZ_00015480"/>
        <obo:IAO_0000115>A fourth-level administrative division of Uganda.</obo:IAO_0000115>
        <oboInOwl:hasOBONamespace>GAZ</oboInOwl:hasOBONamespace>
        <oboInOwl:id>GAZ:00236799</oboInOwl:id>
        <rdfs:label>Bushika Sub-county</rdfs:label>
    </owl:NamedIndividual>
    


    <!-- http://purl.obolibrary.org/obo/GAZ_00236800 -->

    <owl:NamedIndividual rdf:about="http://purl.obolibrary.org/obo/GAZ_00236800">
        <obo:IAO_0000115>A fourth-level administrative division of Uganda.</obo:IAO_0000115>
        <oboInOwl:hasOBONamespace>GAZ</oboInOwl:hasOBONamespace>
        <oboInOwl:id>GAZ:00236800</oboInOwl:id>
        <rdfs:label>Baitambogwe Sub-county</rdfs:label>
    </owl:NamedIndividual>
    


    <!-- http://purl.obolibrary.org/obo/GAZ_00236801 -->

    <owl:NamedIndividual rdf:about="http://purl.obolibrary.org/obo/GAZ_00236801">
        <obo:IAO_0000115>A fourth-level administrative division of Uganda.</obo:IAO_0000115>
        <oboInOwl:hasOBONamespace>GAZ</oboInOwl:hasOBONamespace>
        <oboInOwl:id>GAZ:00236801</oboInOwl:id>
        <rdfs:label>Buwaaya Sub-county</rdfs:label>
    </owl:NamedIndividual>
    


    <!-- http://purl.obolibrary.org/obo/GAZ_00236802 -->

    <owl:NamedIndividual rdf:about="http://purl.obolibrary.org/obo/GAZ_00236802">
        <obo:IAO_0000115>A fourth-level administrative division of Uganda.</obo:IAO_0000115>
        <oboInOwl:hasOBONamespace>GAZ</oboInOwl:hasOBONamespace>
        <oboInOwl:id>GAZ:00236802</oboInOwl:id>
        <rdfs:label>Immanyiro Sub-county</rdfs:label>
    </owl:NamedIndividual>
    


    <!-- http://purl.obolibrary.org/obo/GAZ_00236803 -->

    <owl:NamedIndividual rdf:about="http://purl.obolibrary.org/obo/GAZ_00236803">
        <obo:IAO_0000115>A fourth-level administrative division of Uganda.</obo:IAO_0000115>
        <oboInOwl:hasOBONamespace>GAZ</oboInOwl:hasOBONamespace>
        <oboInOwl:id>GAZ:00236803</oboInOwl:id>
        <rdfs:label>Kigandalo Sub-county</rdfs:label>
    </owl:NamedIndividual>
    


    <!-- http://purl.obolibrary.org/obo/GAZ_00236804 -->

    <owl:NamedIndividual rdf:about="http://purl.obolibrary.org/obo/GAZ_00236804">
        <obo:IAO_0000115>A fourth-level administrative division of Uganda.</obo:IAO_0000115>
        <oboInOwl:hasOBONamespace>GAZ</oboInOwl:hasOBONamespace>
        <oboInOwl:id>GAZ:00236804</oboInOwl:id>
        <rdfs:label>Kityerera Sub-county</rdfs:label>
    </owl:NamedIndividual>
    


    <!-- http://purl.obolibrary.org/obo/GAZ_00236805 -->

    <owl:NamedIndividual rdf:about="http://purl.obolibrary.org/obo/GAZ_00236805">
        <obo:IAO_0000115>A fourth-level administrative division of Uganda.</obo:IAO_0000115>
        <oboInOwl:hasOBONamespace>GAZ</oboInOwl:hasOBONamespace>
        <oboInOwl:id>GAZ:00236805</oboInOwl:id>
        <rdfs:label>Malongo Sub-county</rdfs:label>
    </owl:NamedIndividual>
    


    <!-- http://purl.obolibrary.org/obo/GAZ_00236806 -->

    <owl:NamedIndividual rdf:about="http://purl.obolibrary.org/obo/GAZ_00236806">
        <obo:IAO_0000115>A fourth-level administrative division of Uganda.</obo:IAO_0000115>
        <oboInOwl:hasOBONamespace>GAZ</oboInOwl:hasOBONamespace>
        <oboInOwl:id>GAZ:00236806</oboInOwl:id>
        <rdfs:label>Mayuge Town</rdfs:label>
    </owl:NamedIndividual>
    


    <!-- http://purl.obolibrary.org/obo/GAZ_00236807 -->

    <owl:NamedIndividual rdf:about="http://purl.obolibrary.org/obo/GAZ_00236807">
        <obo:RO_0001025 rdf:resource="http://purl.obolibrary.org/obo/GAZ_00015482"/>
        <obo:IAO_0000115>A fourth-level administrative division of Uganda.</obo:IAO_0000115>
        <oboInOwl:hasOBONamespace>GAZ</oboInOwl:hasOBONamespace>
        <oboInOwl:id>GAZ:00236807</oboInOwl:id>
        <rdfs:label>Bufumbo Sub-county</rdfs:label>
    </owl:NamedIndividual>
    


    <!-- http://purl.obolibrary.org/obo/GAZ_00236808 -->

    <owl:NamedIndividual rdf:about="http://purl.obolibrary.org/obo/GAZ_00236808">
        <obo:RO_0001025 rdf:resource="http://purl.obolibrary.org/obo/GAZ_00015482"/>
        <obo:IAO_0000115>A fourth-level administrative division of Uganda.</obo:IAO_0000115>
        <oboInOwl:hasOBONamespace>GAZ</oboInOwl:hasOBONamespace>
        <oboInOwl:id>GAZ:00236808</oboInOwl:id>
        <rdfs:label>Bukonde Sub-county</rdfs:label>
    </owl:NamedIndividual>
    


    <!-- http://purl.obolibrary.org/obo/GAZ_00236809 -->

    <owl:NamedIndividual rdf:about="http://purl.obolibrary.org/obo/GAZ_00236809">
        <obo:RO_0001025 rdf:resource="http://purl.obolibrary.org/obo/GAZ_00015482"/>
        <obo:IAO_0000115>A fourth-level administrative division of Uganda.</obo:IAO_0000115>
        <oboInOwl:hasOBONamespace>GAZ</oboInOwl:hasOBONamespace>
        <oboInOwl:id>GAZ:00236809</oboInOwl:id>
        <rdfs:label>Bukyiende Sub-county</rdfs:label>
    </owl:NamedIndividual>
    


    <!-- http://purl.obolibrary.org/obo/GAZ_00236810 -->

    <owl:NamedIndividual rdf:about="http://purl.obolibrary.org/obo/GAZ_00236810">
        <obo:RO_0001025 rdf:resource="http://purl.obolibrary.org/obo/GAZ_00015482"/>
        <obo:IAO_0000115>A fourth-level administrative division of Uganda.</obo:IAO_0000115>
        <oboInOwl:hasOBONamespace>GAZ</oboInOwl:hasOBONamespace>
        <oboInOwl:id>GAZ:00236810</oboInOwl:id>
        <rdfs:label>Bungokho Sub-county</rdfs:label>
    </owl:NamedIndividual>
    


    <!-- http://purl.obolibrary.org/obo/GAZ_00236811 -->

    <owl:NamedIndividual rdf:about="http://purl.obolibrary.org/obo/GAZ_00236811">
        <obo:RO_0001025 rdf:resource="http://purl.obolibrary.org/obo/GAZ_00015482"/>
        <obo:IAO_0000115>A fourth-level administrative division of Uganda.</obo:IAO_0000115>
        <oboInOwl:hasOBONamespace>GAZ</oboInOwl:hasOBONamespace>
        <oboInOwl:id>GAZ:00236811</oboInOwl:id>
        <rdfs:label>Bungokho-Mutoto Sub-county</rdfs:label>
    </owl:NamedIndividual>
    


    <!-- http://purl.obolibrary.org/obo/GAZ_00236812 -->

    <owl:NamedIndividual rdf:about="http://purl.obolibrary.org/obo/GAZ_00236812">
        <obo:RO_0001025 rdf:resource="http://purl.obolibrary.org/obo/GAZ_00015482"/>
        <obo:IAO_0000115>A fourth-level administrative division of Uganda.</obo:IAO_0000115>
        <oboInOwl:hasOBONamespace>GAZ</oboInOwl:hasOBONamespace>
        <oboInOwl:id>GAZ:00236812</oboInOwl:id>
        <rdfs:label>Busano Sub-county</rdfs:label>
    </owl:NamedIndividual>
    


    <!-- http://purl.obolibrary.org/obo/GAZ_00236813 -->

    <owl:NamedIndividual rdf:about="http://purl.obolibrary.org/obo/GAZ_00236813">
        <obo:RO_0001025 rdf:resource="http://purl.obolibrary.org/obo/GAZ_00015482"/>
        <obo:IAO_0000115>A fourth-level administrative division of Uganda.</obo:IAO_0000115>
        <oboInOwl:hasOBONamespace>GAZ</oboInOwl:hasOBONamespace>
        <oboInOwl:id>GAZ:00236813</oboInOwl:id>
        <rdfs:label>Busiu Sub-county</rdfs:label>
    </owl:NamedIndividual>
    


    <!-- http://purl.obolibrary.org/obo/GAZ_00236814 -->

    <owl:NamedIndividual rdf:about="http://purl.obolibrary.org/obo/GAZ_00236814">
        <obo:RO_0001025 rdf:resource="http://purl.obolibrary.org/obo/GAZ_00015482"/>
        <obo:IAO_0000115>A fourth-level administrative division of Uganda.</obo:IAO_0000115>
        <oboInOwl:hasOBONamespace>GAZ</oboInOwl:hasOBONamespace>
        <oboInOwl:id>GAZ:00236814</oboInOwl:id>
        <rdfs:label>Busoba Sub-county</rdfs:label>
    </owl:NamedIndividual>
    


    <!-- http://purl.obolibrary.org/obo/GAZ_00236815 -->

    <owl:NamedIndividual rdf:about="http://purl.obolibrary.org/obo/GAZ_00236815">
        <obo:RO_0001025 rdf:resource="http://purl.obolibrary.org/obo/GAZ_00015482"/>
        <obo:IAO_0000115>A fourth-level administrative division of Uganda.</obo:IAO_0000115>
        <oboInOwl:hasOBONamespace>GAZ</oboInOwl:hasOBONamespace>
        <oboInOwl:id>GAZ:00236815</oboInOwl:id>
        <rdfs:label>Nakaloke Sub-county</rdfs:label>
    </owl:NamedIndividual>
    


    <!-- http://purl.obolibrary.org/obo/GAZ_00236816 -->

    <owl:NamedIndividual rdf:about="http://purl.obolibrary.org/obo/GAZ_00236816">
        <obo:RO_0001025 rdf:resource="http://purl.obolibrary.org/obo/GAZ_00015482"/>
        <obo:IAO_0000115>A fourth-level administrative division of Uganda.</obo:IAO_0000115>
        <oboInOwl:hasOBONamespace>GAZ</oboInOwl:hasOBONamespace>
        <oboInOwl:id>GAZ:00236816</oboInOwl:id>
        <rdfs:label>Namanyonyi Sub-county</rdfs:label>
    </owl:NamedIndividual>
    


    <!-- http://purl.obolibrary.org/obo/GAZ_00236817 -->

    <owl:NamedIndividual rdf:about="http://purl.obolibrary.org/obo/GAZ_00236817">
        <obo:RO_0001025 rdf:resource="http://purl.obolibrary.org/obo/GAZ_00015482"/>
        <obo:IAO_0000115>A fourth-level administrative division of Uganda.</obo:IAO_0000115>
        <oboInOwl:hasOBONamespace>GAZ</oboInOwl:hasOBONamespace>
        <oboInOwl:id>GAZ:00236817</oboInOwl:id>
        <rdfs:label>Wanale Sub-county</rdfs:label>
    </owl:NamedIndividual>
    


    <!-- http://purl.obolibrary.org/obo/GAZ_00236818 -->

    <owl:NamedIndividual rdf:about="http://purl.obolibrary.org/obo/GAZ_00236818">
        <obo:RO_0001025 rdf:resource="http://purl.obolibrary.org/obo/GAZ_00015483"/>
        <obo:IAO_0000115>A fourth-level administrative division of Uganda.</obo:IAO_0000115>
        <oboInOwl:hasOBONamespace>GAZ</oboInOwl:hasOBONamespace>
        <oboInOwl:id>GAZ:00236818</oboInOwl:id>
        <rdfs:label>Mbale Industrial Division</rdfs:label>
    </owl:NamedIndividual>
    


    <!-- http://purl.obolibrary.org/obo/GAZ_00236819 -->

    <owl:NamedIndividual rdf:about="http://purl.obolibrary.org/obo/GAZ_00236819">
        <obo:RO_0001025 rdf:resource="http://purl.obolibrary.org/obo/GAZ_00015483"/>
        <obo:IAO_0000115>A fourth-level administrative division of Uganda.</obo:IAO_0000115>
        <oboInOwl:hasOBONamespace>GAZ</oboInOwl:hasOBONamespace>
        <oboInOwl:id>GAZ:00236819</oboInOwl:id>
        <rdfs:label>Mbale Northern Division</rdfs:label>
    </owl:NamedIndividual>
    


    <!-- http://purl.obolibrary.org/obo/GAZ_00236820 -->

    <owl:NamedIndividual rdf:about="http://purl.obolibrary.org/obo/GAZ_00236820">
        <obo:RO_0001025 rdf:resource="http://purl.obolibrary.org/obo/GAZ_00015483"/>
        <obo:IAO_0000115>A fourth-level administrative division of Uganda.</obo:IAO_0000115>
        <oboInOwl:hasOBONamespace>GAZ</oboInOwl:hasOBONamespace>
        <oboInOwl:id>GAZ:00236820</oboInOwl:id>
        <rdfs:label>Mbale Wanale Division</rdfs:label>
    </owl:NamedIndividual>
    


    <!-- http://purl.obolibrary.org/obo/GAZ_00236821 -->

    <owl:NamedIndividual rdf:about="http://purl.obolibrary.org/obo/GAZ_00236821">
        <rdf:type rdf:resource="http://purl.obolibrary.org/obo/ENVO_00000004"/>
        <obo:RO_0001025 rdf:resource="http://purl.obolibrary.org/obo/GAZ_00015363"/>
        <obo:IAO_0000115>An administrative division of Namutumba District.</obo:IAO_0000115>
        <oboInOwl:hasOBONamespace>GAZ</oboInOwl:hasOBONamespace>
        <oboInOwl:id>GAZ:00236821</oboInOwl:id>
        <rdfs:label>Bulange Sub-county</rdfs:label>
    </owl:NamedIndividual>
    


    <!-- http://purl.obolibrary.org/obo/GAZ_00236822 -->

    <owl:NamedIndividual rdf:about="http://purl.obolibrary.org/obo/GAZ_00236822">
        <rdf:type rdf:resource="http://purl.obolibrary.org/obo/ENVO_00000004"/>
        <obo:RO_0001025 rdf:resource="http://purl.obolibrary.org/obo/GAZ_00015363"/>
        <obo:IAO_0000115>An administrative division of Namutumba District.</obo:IAO_0000115>
        <oboInOwl:hasOBONamespace>GAZ</oboInOwl:hasOBONamespace>
        <oboInOwl:id>GAZ:00236822</oboInOwl:id>
        <rdfs:label>Ivukula Sub-county</rdfs:label>
    </owl:NamedIndividual>
    


    <!-- http://purl.obolibrary.org/obo/GAZ_00236823 -->

    <owl:NamedIndividual rdf:about="http://purl.obolibrary.org/obo/GAZ_00236823">
        <rdf:type rdf:resource="http://purl.obolibrary.org/obo/ENVO_00000004"/>
        <obo:RO_0001025 rdf:resource="http://purl.obolibrary.org/obo/GAZ_00015363"/>
        <obo:IAO_0000115>An administrative division of Namutumba District.</obo:IAO_0000115>
        <oboInOwl:hasOBONamespace>GAZ</oboInOwl:hasOBONamespace>
        <oboInOwl:id>GAZ:00236823</oboInOwl:id>
        <rdfs:label>Kibaale Sub-county</rdfs:label>
    </owl:NamedIndividual>
    


    <!-- http://purl.obolibrary.org/obo/GAZ_00236824 -->

    <owl:NamedIndividual rdf:about="http://purl.obolibrary.org/obo/GAZ_00236824">
        <rdf:type rdf:resource="http://purl.obolibrary.org/obo/ENVO_00000004"/>
        <obo:RO_0001025 rdf:resource="http://purl.obolibrary.org/obo/GAZ_00015363"/>
        <obo:IAO_0000115>An administrative division of Namutumba District.</obo:IAO_0000115>
        <oboInOwl:hasOBONamespace>GAZ</oboInOwl:hasOBONamespace>
        <oboInOwl:id>GAZ:00236824</oboInOwl:id>
        <rdfs:label>Magada Sub-county</rdfs:label>
    </owl:NamedIndividual>
    


    <!-- http://purl.obolibrary.org/obo/GAZ_00236825 -->

    <owl:NamedIndividual rdf:about="http://purl.obolibrary.org/obo/GAZ_00236825">
        <rdf:type rdf:resource="http://purl.obolibrary.org/obo/ENVO_00000004"/>
        <obo:RO_0001025 rdf:resource="http://purl.obolibrary.org/obo/GAZ_00015363"/>
        <obo:IAO_0000115>An administrative division of Namutumba District.</obo:IAO_0000115>
        <oboInOwl:hasOBONamespace>GAZ</oboInOwl:hasOBONamespace>
        <oboInOwl:id>GAZ:00236825</oboInOwl:id>
        <rdfs:label>Namutumba Sub-county</rdfs:label>
    </owl:NamedIndividual>
    


    <!-- http://purl.obolibrary.org/obo/GAZ_00236826 -->

    <owl:NamedIndividual rdf:about="http://purl.obolibrary.org/obo/GAZ_00236826">
        <rdf:type rdf:resource="http://purl.obolibrary.org/obo/ENVO_00000004"/>
        <obo:RO_0001025 rdf:resource="http://purl.obolibrary.org/obo/GAZ_00015363"/>
        <obo:IAO_0000115>An administrative division of Namutumba District.</obo:IAO_0000115>
        <oboInOwl:hasOBONamespace>GAZ</oboInOwl:hasOBONamespace>
        <oboInOwl:id>GAZ:00236826</oboInOwl:id>
        <rdfs:label>Namutumba Town</rdfs:label>
    </owl:NamedIndividual>
    


    <!-- http://purl.obolibrary.org/obo/GAZ_00236827 -->

    <owl:NamedIndividual rdf:about="http://purl.obolibrary.org/obo/GAZ_00236827">
        <rdf:type rdf:resource="http://purl.obolibrary.org/obo/ENVO_00000004"/>
        <obo:RO_0001025 rdf:resource="http://purl.obolibrary.org/obo/GAZ_00015363"/>
        <obo:IAO_0000115>An administrative division of Namutumba District.</obo:IAO_0000115>
        <oboInOwl:hasOBONamespace>GAZ</oboInOwl:hasOBONamespace>
        <oboInOwl:id>GAZ:00236827</oboInOwl:id>
        <rdfs:label>Nsinze Sub-county</rdfs:label>
    </owl:NamedIndividual>
    


    <!-- http://purl.obolibrary.org/obo/GAZ_00236828 -->

    <owl:NamedIndividual rdf:about="http://purl.obolibrary.org/obo/GAZ_00236828">
        <obo:RO_0001025 rdf:resource="http://purl.obolibrary.org/obo/GAZ_00236836"/>
        <obo:IAO_0000115>A lake.</obo:IAO_0000115>
        <oboInOwl:hasOBONamespace>GAZ</oboInOwl:hasOBONamespace>
        <oboInOwl:id>GAZ:00236828</oboInOwl:id>
        <rdfs:label>Lake Lemwa</rdfs:label>
    </owl:NamedIndividual>
    


    <!-- http://purl.obolibrary.org/obo/GAZ_00236829 -->

    <owl:NamedIndividual rdf:about="http://purl.obolibrary.org/obo/GAZ_00236829">
        <obo:RO_0001025 rdf:resource="http://purl.obolibrary.org/obo/GAZ_00236836"/>
        <obo:IAO_0000115>A lake.</obo:IAO_0000115>
        <oboInOwl:hasOBONamespace>GAZ</oboInOwl:hasOBONamespace>
        <oboInOwl:id>GAZ:00236829</oboInOwl:id>
        <rdfs:label>Lake Kawi</rdfs:label>
    </owl:NamedIndividual>
    


    <!-- http://purl.obolibrary.org/obo/GAZ_00236830 -->

    <owl:NamedIndividual rdf:about="http://purl.obolibrary.org/obo/GAZ_00236830">
        <obo:RO_0001025 rdf:resource="http://purl.obolibrary.org/obo/GAZ_00236836"/>
        <obo:IAO_0000115>A lake.</obo:IAO_0000115>
        <oboInOwl:hasOBONamespace>GAZ</oboInOwl:hasOBONamespace>
        <oboInOwl:id>GAZ:00236830</oboInOwl:id>
        <rdfs:label>Lake Nakwa</rdfs:label>
    </owl:NamedIndividual>
    


    <!-- http://purl.obolibrary.org/obo/GAZ_00236831 -->

    <owl:NamedIndividual rdf:about="http://purl.obolibrary.org/obo/GAZ_00236831">
        <obo:RO_0001025 rdf:resource="http://purl.obolibrary.org/obo/GAZ_00236836"/>
        <obo:IAO_0000115>A lake.</obo:IAO_0000115>
        <oboInOwl:hasOBONamespace>GAZ</oboInOwl:hasOBONamespace>
        <oboInOwl:id>GAZ:00236831</oboInOwl:id>
        <rdfs:label>Lake Meito</rdfs:label>
    </owl:NamedIndividual>
    


    <!-- http://purl.obolibrary.org/obo/GAZ_00236832 -->

    <owl:NamedIndividual rdf:about="http://purl.obolibrary.org/obo/GAZ_00236832">
        <obo:RO_0001025 rdf:resource="http://purl.obolibrary.org/obo/GAZ_00236836"/>
        <obo:IAO_0000115>A lake.</obo:IAO_0000115>
        <oboInOwl:hasOBONamespace>GAZ</oboInOwl:hasOBONamespace>
        <oboInOwl:id>GAZ:00236832</oboInOwl:id>
        <rdfs:label>Lake Geme</rdfs:label>
    </owl:NamedIndividual>
    


    <!-- http://purl.obolibrary.org/obo/GAZ_00236833 -->

    <owl:NamedIndividual rdf:about="http://purl.obolibrary.org/obo/GAZ_00236833">
        <obo:RO_0001025 rdf:resource="http://purl.obolibrary.org/obo/GAZ_00236836"/>
        <obo:IAO_0000115>A lake.</obo:IAO_0000115>
        <oboInOwl:hasOBONamespace>GAZ</oboInOwl:hasOBONamespace>
        <oboInOwl:id>GAZ:00236833</oboInOwl:id>
        <rdfs:label>Lake Omunuo</rdfs:label>
    </owl:NamedIndividual>
    


    <!-- http://purl.obolibrary.org/obo/GAZ_00236834 -->

    <owl:NamedIndividual rdf:about="http://purl.obolibrary.org/obo/GAZ_00236834">
        <obo:RO_0001025 rdf:resource="http://purl.obolibrary.org/obo/GAZ_00236836"/>
        <obo:IAO_0000115>A lake.</obo:IAO_0000115>
        <oboInOwl:hasOBONamespace>GAZ</oboInOwl:hasOBONamespace>
        <oboInOwl:id>GAZ:00236834</oboInOwl:id>
        <rdfs:label>Lake Nyanzala</rdfs:label>
    </owl:NamedIndividual>
    


    <!-- http://purl.obolibrary.org/obo/GAZ_00236835 -->

    <owl:NamedIndividual rdf:about="http://purl.obolibrary.org/obo/GAZ_00236835">
        <obo:RO_0001025 rdf:resource="http://purl.obolibrary.org/obo/GAZ_00236836"/>
        <obo:IAO_0000115>A lake.</obo:IAO_0000115>
        <oboInOwl:hasOBONamespace>GAZ</oboInOwl:hasOBONamespace>
        <oboInOwl:id>GAZ:00236835</oboInOwl:id>
        <rdfs:label>Lake Nyaguo</rdfs:label>
    </owl:NamedIndividual>
    


    <!-- http://purl.obolibrary.org/obo/GAZ_00236836 -->

    <owl:NamedIndividual rdf:about="http://purl.obolibrary.org/obo/GAZ_00236836">
        <obo:RO_0001025 rdf:resource="http://purl.obolibrary.org/obo/GAZ_00015370"/>
        <obo:IAO_0000115>A third-level administrative division of Uganda.</obo:IAO_0000115>
        <oboInOwl:hasOBONamespace>GAZ</oboInOwl:hasOBONamespace>
        <oboInOwl:id>GAZ:00236836</oboInOwl:id>
        <rdfs:label>Pallisa County</rdfs:label>
    </owl:NamedIndividual>
    


    <!-- http://purl.obolibrary.org/obo/GAZ_00236837 -->

    <owl:NamedIndividual rdf:about="http://purl.obolibrary.org/obo/GAZ_00236837">
        <obo:RO_0001025 rdf:resource="http://purl.obolibrary.org/obo/GAZ_00236836"/>
        <obo:IAO_0000115>A fourth-level administrative division of Uganda.</obo:IAO_0000115>
        <oboInOwl:hasOBONamespace>GAZ</oboInOwl:hasOBONamespace>
        <oboInOwl:id>GAZ:00236837</oboInOwl:id>
        <rdfs:label>Agule Sub-county</rdfs:label>
    </owl:NamedIndividual>
    


    <!-- http://purl.obolibrary.org/obo/GAZ_00236838 -->

    <owl:NamedIndividual rdf:about="http://purl.obolibrary.org/obo/GAZ_00236838">
        <obo:RO_0001025 rdf:resource="http://purl.obolibrary.org/obo/GAZ_00236836"/>
        <obo:IAO_0000115>A fourth-level administrative division of Uganda.</obo:IAO_0000115>
        <oboInOwl:hasOBONamespace>GAZ</oboInOwl:hasOBONamespace>
        <oboInOwl:id>GAZ:00236838</oboInOwl:id>
        <rdfs:label>Apopong Sub-county</rdfs:label>
    </owl:NamedIndividual>
    


    <!-- http://purl.obolibrary.org/obo/GAZ_00236839 -->

    <owl:NamedIndividual rdf:about="http://purl.obolibrary.org/obo/GAZ_00236839">
        <obo:RO_0001025 rdf:resource="http://purl.obolibrary.org/obo/GAZ_00236836"/>
        <obo:IAO_0000115>A fourth-level administrative division of Uganda.</obo:IAO_0000115>
        <oboInOwl:hasOBONamespace>GAZ</oboInOwl:hasOBONamespace>
        <oboInOwl:id>GAZ:00236839</oboInOwl:id>
        <rdfs:label>Gogonyo Sub-county</rdfs:label>
    </owl:NamedIndividual>
    


    <!-- http://purl.obolibrary.org/obo/GAZ_00236840 -->

    <owl:NamedIndividual rdf:about="http://purl.obolibrary.org/obo/GAZ_00236840">
        <obo:RO_0001025 rdf:resource="http://purl.obolibrary.org/obo/GAZ_00236836"/>
        <obo:IAO_0000115>A fourth-level administrative division of Uganda.</obo:IAO_0000115>
        <oboInOwl:hasOBONamespace>GAZ</oboInOwl:hasOBONamespace>
        <oboInOwl:id>GAZ:00236840</oboInOwl:id>
        <rdfs:label>Kameke Sub-county</rdfs:label>
    </owl:NamedIndividual>
    


    <!-- http://purl.obolibrary.org/obo/GAZ_00236841 -->

    <owl:NamedIndividual rdf:about="http://purl.obolibrary.org/obo/GAZ_00236841">
        <obo:RO_0001025 rdf:resource="http://purl.obolibrary.org/obo/GAZ_00236836"/>
        <obo:IAO_0000115>A fourth-level administrative division of Uganda.</obo:IAO_0000115>
        <oboInOwl:hasOBONamespace>GAZ</oboInOwl:hasOBONamespace>
        <oboInOwl:id>GAZ:00236841</oboInOwl:id>
        <rdfs:label>Kasodo Sub-county</rdfs:label>
    </owl:NamedIndividual>
    


    <!-- http://purl.obolibrary.org/obo/GAZ_00236842 -->

    <owl:NamedIndividual rdf:about="http://purl.obolibrary.org/obo/GAZ_00236842">
        <obo:RO_0001025 rdf:resource="http://purl.obolibrary.org/obo/GAZ_00236836"/>
        <obo:IAO_0000115>A fourth-level administrative division of Uganda.</obo:IAO_0000115>
        <oboInOwl:hasOBONamespace>GAZ</oboInOwl:hasOBONamespace>
        <oboInOwl:id>GAZ:00236842</oboInOwl:id>
        <rdfs:label>Pallisa Sub-county</rdfs:label>
    </owl:NamedIndividual>
    


    <!-- http://purl.obolibrary.org/obo/GAZ_00236843 -->

    <owl:NamedIndividual rdf:about="http://purl.obolibrary.org/obo/GAZ_00236843">
        <obo:RO_0001025 rdf:resource="http://purl.obolibrary.org/obo/GAZ_00236836"/>
        <obo:IAO_0000115>A fourth-level administrative division of Uganda.</obo:IAO_0000115>
        <oboInOwl:hasOBONamespace>GAZ</oboInOwl:hasOBONamespace>
        <oboInOwl:id>GAZ:00236843</oboInOwl:id>
        <rdfs:label>Pallisa Town</rdfs:label>
    </owl:NamedIndividual>
    


    <!-- http://purl.obolibrary.org/obo/GAZ_00236844 -->

    <owl:NamedIndividual rdf:about="http://purl.obolibrary.org/obo/GAZ_00236844">
        <obo:RO_0001025 rdf:resource="http://purl.obolibrary.org/obo/GAZ_00236836"/>
        <obo:IAO_0000115>A fourth-level administrative division of Uganda.</obo:IAO_0000115>
        <oboInOwl:hasOBONamespace>GAZ</oboInOwl:hasOBONamespace>
        <oboInOwl:id>GAZ:00236844</oboInOwl:id>
        <rdfs:label>Puti-puti Sub-county</rdfs:label>
    </owl:NamedIndividual>
    


    <!-- http://purl.obolibrary.org/obo/GAZ_00236845 -->

    <owl:NamedIndividual rdf:about="http://purl.obolibrary.org/obo/GAZ_00236845">
        <obo:RO_0001025 rdf:resource="http://purl.obolibrary.org/obo/GAZ_00236836"/>
        <obo:IAO_0000115>A fourth-level administrative division of Uganda.</obo:IAO_0000115>
        <oboInOwl:hasOBONamespace>GAZ</oboInOwl:hasOBONamespace>
        <oboInOwl:id>GAZ:00236845</oboInOwl:id>
        <rdfs:label>Kamuge Sub-county</rdfs:label>
    </owl:NamedIndividual>
    


    <!-- http://purl.obolibrary.org/obo/GAZ_00236846 -->

    <owl:NamedIndividual rdf:about="http://purl.obolibrary.org/obo/GAZ_00236846">
        <obo:RO_0001025 rdf:resource="http://purl.obolibrary.org/obo/GAZ_00015421"/>
        <obo:IAO_0000115>A fourth-level administrative division of Uganda.</obo:IAO_0000115>
        <oboInOwl:hasOBONamespace>GAZ</oboInOwl:hasOBONamespace>
        <oboInOwl:id>GAZ:00236846</oboInOwl:id>
        <rdfs:label>Buhugu Sub-county</rdfs:label>
    </owl:NamedIndividual>
    


    <!-- http://purl.obolibrary.org/obo/GAZ_00236847 -->

    <owl:NamedIndividual rdf:about="http://purl.obolibrary.org/obo/GAZ_00236847">
        <obo:RO_0001025 rdf:resource="http://purl.obolibrary.org/obo/GAZ_00015421"/>
        <obo:IAO_0000115>A fourth-level administrative division of Uganda.</obo:IAO_0000115>
        <oboInOwl:hasOBONamespace>GAZ</oboInOwl:hasOBONamespace>
        <oboInOwl:id>GAZ:00236847</oboInOwl:id>
        <rdfs:label>Bumasifwa Sub-county</rdfs:label>
    </owl:NamedIndividual>
    


    <!-- http://purl.obolibrary.org/obo/GAZ_00236848 -->

    <owl:NamedIndividual rdf:about="http://purl.obolibrary.org/obo/GAZ_00236848">
        <obo:RO_0001025 rdf:resource="http://purl.obolibrary.org/obo/GAZ_00015421"/>
        <obo:IAO_0000115>A fourth-level administrative division of Uganda.</obo:IAO_0000115>
        <oboInOwl:hasOBONamespace>GAZ</oboInOwl:hasOBONamespace>
        <oboInOwl:id>GAZ:00236848</oboInOwl:id>
        <rdfs:label>Busulani Sub-county</rdfs:label>
    </owl:NamedIndividual>
    


    <!-- http://purl.obolibrary.org/obo/GAZ_00236849 -->

    <owl:NamedIndividual rdf:about="http://purl.obolibrary.org/obo/GAZ_00236849">
        <obo:RO_0001025 rdf:resource="http://purl.obolibrary.org/obo/GAZ_00015421"/>
        <obo:IAO_0000115>A fourth-level administrative division of Uganda.</obo:IAO_0000115>
        <oboInOwl:hasOBONamespace>GAZ</oboInOwl:hasOBONamespace>
        <oboInOwl:id>GAZ:00236849</oboInOwl:id>
        <rdfs:label>Butandiga Sub-county</rdfs:label>
    </owl:NamedIndividual>
    


    <!-- http://purl.obolibrary.org/obo/GAZ_00236850 -->

    <owl:NamedIndividual rdf:about="http://purl.obolibrary.org/obo/GAZ_00236850">
        <obo:RO_0001025 rdf:resource="http://purl.obolibrary.org/obo/GAZ_00015421"/>
        <obo:IAO_0000115>A fourth-level administrative division of Uganda.</obo:IAO_0000115>
        <oboInOwl:hasOBONamespace>GAZ</oboInOwl:hasOBONamespace>
        <oboInOwl:id>GAZ:00236850</oboInOwl:id>
        <rdfs:label>Buteza Sub-county</rdfs:label>
    </owl:NamedIndividual>
    


    <!-- http://purl.obolibrary.org/obo/GAZ_00236851 -->

    <owl:NamedIndividual rdf:about="http://purl.obolibrary.org/obo/GAZ_00236851">
        <obo:RO_0001025 rdf:resource="http://purl.obolibrary.org/obo/GAZ_00015421"/>
        <obo:IAO_0000115>A fourth-level administrative division of Uganda.</obo:IAO_0000115>
        <oboInOwl:hasOBONamespace>GAZ</oboInOwl:hasOBONamespace>
        <oboInOwl:id>GAZ:00236851</oboInOwl:id>
        <rdfs:label>Buwalasi Sub-county</rdfs:label>
    </owl:NamedIndividual>
    


    <!-- http://purl.obolibrary.org/obo/GAZ_00236852 -->

    <owl:NamedIndividual rdf:about="http://purl.obolibrary.org/obo/GAZ_00236852">
        <obo:RO_0001025 rdf:resource="http://purl.obolibrary.org/obo/GAZ_00015421"/>
        <obo:IAO_0000115>A fourth-level administrative division of Uganda.</obo:IAO_0000115>
        <oboInOwl:hasOBONamespace>GAZ</oboInOwl:hasOBONamespace>
        <oboInOwl:id>GAZ:00236852</oboInOwl:id>
        <rdfs:label>Buyobo Sub-county</rdfs:label>
    </owl:NamedIndividual>
    


    <!-- http://purl.obolibrary.org/obo/GAZ_00236853 -->

    <owl:NamedIndividual rdf:about="http://purl.obolibrary.org/obo/GAZ_00236853">
        <obo:RO_0001025 rdf:resource="http://purl.obolibrary.org/obo/GAZ_00015421"/>
        <obo:IAO_0000115>A fourth-level administrative division of Uganda.</obo:IAO_0000115>
        <oboInOwl:hasOBONamespace>GAZ</oboInOwl:hasOBONamespace>
        <oboInOwl:id>GAZ:00236853</oboInOwl:id>
        <rdfs:label>Sironko Town</rdfs:label>
    </owl:NamedIndividual>
    


    <!-- http://purl.obolibrary.org/obo/GAZ_00236854 -->

    <owl:NamedIndividual rdf:about="http://purl.obolibrary.org/obo/GAZ_00236854">
        <obo:RO_0001025 rdf:resource="http://purl.obolibrary.org/obo/GAZ_00015421"/>
        <obo:IAO_0000115>A fourth-level administrative division of Uganda.</obo:IAO_0000115>
        <oboInOwl:hasOBONamespace>GAZ</oboInOwl:hasOBONamespace>
        <oboInOwl:id>GAZ:00236854</oboInOwl:id>
        <rdfs:label>Zesui Sub-county</rdfs:label>
    </owl:NamedIndividual>
    


    <!-- http://purl.obolibrary.org/obo/GAZ_00236855 -->

    <owl:NamedIndividual rdf:about="http://purl.obolibrary.org/obo/GAZ_00236855">
        <obo:RO_0001025 rdf:resource="http://purl.obolibrary.org/obo/GAZ_00015421"/>
        <obo:IAO_0000115>A fourth-level administrative division of Uganda.</obo:IAO_0000115>
        <oboInOwl:hasOBONamespace>GAZ</oboInOwl:hasOBONamespace>
        <oboInOwl:id>GAZ:00236855</oboInOwl:id>
        <rdfs:label>Bukhulo Sub-county</rdfs:label>
    </owl:NamedIndividual>
    


    <!-- http://purl.obolibrary.org/obo/GAZ_00236856 -->

    <owl:NamedIndividual rdf:about="http://purl.obolibrary.org/obo/GAZ_00236856">
        <obo:RO_0001025 rdf:resource="http://purl.obolibrary.org/obo/GAZ_00015420"/>
        <obo:IAO_0000115>A fourth-level administrative division of Uganda.</obo:IAO_0000115>
        <oboInOwl:hasOBONamespace>GAZ</oboInOwl:hasOBONamespace>
        <oboInOwl:id>GAZ:00236856</oboInOwl:id>
        <rdfs:label>Buginyanya Sub-county</rdfs:label>
    </owl:NamedIndividual>
    


    <!-- http://purl.obolibrary.org/obo/GAZ_00236857 -->

    <owl:NamedIndividual rdf:about="http://purl.obolibrary.org/obo/GAZ_00236857">
        <obo:RO_0001025 rdf:resource="http://purl.obolibrary.org/obo/GAZ_00015420"/>
        <obo:IAO_0000115>A fourth-level administrative division of Uganda.</obo:IAO_0000115>
        <oboInOwl:hasOBONamespace>GAZ</oboInOwl:hasOBONamespace>
        <oboInOwl:id>GAZ:00236857</oboInOwl:id>
        <rdfs:label>Bukhalu Sub-county</rdfs:label>
    </owl:NamedIndividual>
    


    <!-- http://purl.obolibrary.org/obo/GAZ_00236858 -->

    <owl:NamedIndividual rdf:about="http://purl.obolibrary.org/obo/GAZ_00236858">
        <obo:RO_0001025 rdf:resource="http://purl.obolibrary.org/obo/GAZ_00015420"/>
        <obo:IAO_0000115>A fourth-level administrative division of Uganda.</obo:IAO_0000115>
        <oboInOwl:hasOBONamespace>GAZ</oboInOwl:hasOBONamespace>
        <oboInOwl:id>GAZ:00236858</oboInOwl:id>
        <rdfs:label>Bulago Sub-county</rdfs:label>
    </owl:NamedIndividual>
    


    <!-- http://purl.obolibrary.org/obo/GAZ_00236859 -->

    <owl:NamedIndividual rdf:about="http://purl.obolibrary.org/obo/GAZ_00236859">
        <obo:RO_0001025 rdf:resource="http://purl.obolibrary.org/obo/GAZ_00015420"/>
        <obo:IAO_0000115>A fourth-level administrative division of Uganda.</obo:IAO_0000115>
        <oboInOwl:hasOBONamespace>GAZ</oboInOwl:hasOBONamespace>
        <oboInOwl:id>GAZ:00236859</oboInOwl:id>
        <rdfs:label>Bulegeni Sub-county</rdfs:label>
    </owl:NamedIndividual>
    


    <!-- http://purl.obolibrary.org/obo/GAZ_00236860 -->

    <owl:NamedIndividual rdf:about="http://purl.obolibrary.org/obo/GAZ_00236860">
        <obo:RO_0001025 rdf:resource="http://purl.obolibrary.org/obo/GAZ_00015420"/>
        <obo:IAO_0000115>A fourth-level administrative division of Uganda.</obo:IAO_0000115>
        <oboInOwl:hasOBONamespace>GAZ</oboInOwl:hasOBONamespace>
        <oboInOwl:id>GAZ:00236860</oboInOwl:id>
        <rdfs:label>Buluganya Sub-county</rdfs:label>
    </owl:NamedIndividual>
    


    <!-- http://purl.obolibrary.org/obo/GAZ_00236861 -->

    <owl:NamedIndividual rdf:about="http://purl.obolibrary.org/obo/GAZ_00236861">
        <obo:RO_0001025 rdf:resource="http://purl.obolibrary.org/obo/GAZ_00015420"/>
        <obo:IAO_0000115>A fourth-level administrative division of Uganda.</obo:IAO_0000115>
        <oboInOwl:hasOBONamespace>GAZ</oboInOwl:hasOBONamespace>
        <oboInOwl:id>GAZ:00236861</oboInOwl:id>
        <rdfs:label>Bunambutye Sub-county</rdfs:label>
    </owl:NamedIndividual>
    


    <!-- http://purl.obolibrary.org/obo/GAZ_00236862 -->

    <owl:NamedIndividual rdf:about="http://purl.obolibrary.org/obo/GAZ_00236862">
        <obo:RO_0001025 rdf:resource="http://purl.obolibrary.org/obo/GAZ_00015420"/>
        <obo:IAO_0000115>A fourth-level administrative division of Uganda.</obo:IAO_0000115>
        <oboInOwl:hasOBONamespace>GAZ</oboInOwl:hasOBONamespace>
        <oboInOwl:id>GAZ:00236862</oboInOwl:id>
        <rdfs:label>Masiira Sub-county</rdfs:label>
    </owl:NamedIndividual>
    


    <!-- http://purl.obolibrary.org/obo/GAZ_00236863 -->

    <owl:NamedIndividual rdf:about="http://purl.obolibrary.org/obo/GAZ_00236863">
        <obo:RO_0001025 rdf:resource="http://purl.obolibrary.org/obo/GAZ_00015420"/>
        <obo:IAO_0000115>A fourth-level administrative division of Uganda.</obo:IAO_0000115>
        <oboInOwl:hasOBONamespace>GAZ</oboInOwl:hasOBONamespace>
        <oboInOwl:id>GAZ:00236863</oboInOwl:id>
        <rdfs:label>Muyembe Sub-county</rdfs:label>
    </owl:NamedIndividual>
    


    <!-- http://purl.obolibrary.org/obo/GAZ_00236864 -->

    <owl:NamedIndividual rdf:about="http://purl.obolibrary.org/obo/GAZ_00236864">
        <obo:RO_0001025 rdf:resource="http://purl.obolibrary.org/obo/GAZ_00015420"/>
        <obo:IAO_0000115>A fourth-level administrative division of Uganda.</obo:IAO_0000115>
        <oboInOwl:hasOBONamespace>GAZ</oboInOwl:hasOBONamespace>
        <oboInOwl:id>GAZ:00236864</oboInOwl:id>
        <rdfs:label>Sisiyi Sub-county</rdfs:label>
    </owl:NamedIndividual>
    


    <!-- http://purl.obolibrary.org/obo/GAZ_00236865 -->

    <owl:NamedIndividual rdf:about="http://purl.obolibrary.org/obo/GAZ_00236865">
        <obo:RO_0001025 rdf:resource="http://purl.obolibrary.org/obo/GAZ_00015419"/>
        <obo:IAO_0000115>A fourth-level administrative division of Uganda.</obo:IAO_0000115>
        <oboInOwl:hasOBONamespace>GAZ</oboInOwl:hasOBONamespace>
        <oboInOwl:id>GAZ:00236865</oboInOwl:id>
        <rdfs:label>Bugondo Sub-count</rdfs:label>
    </owl:NamedIndividual>
    


    <!-- http://purl.obolibrary.org/obo/GAZ_00236866 -->

    <owl:NamedIndividual rdf:about="http://purl.obolibrary.org/obo/GAZ_00236866">
        <obo:RO_0001025 rdf:resource="http://purl.obolibrary.org/obo/GAZ_00015419"/>
        <obo:IAO_0000115>A fourth-level administrative division of Uganda.</obo:IAO_0000115>
        <oboInOwl:hasOBONamespace>GAZ</oboInOwl:hasOBONamespace>
        <oboInOwl:id>GAZ:00236866</oboInOwl:id>
        <rdfs:label>Kadungulu Sub-county</rdfs:label>
    </owl:NamedIndividual>
    


    <!-- http://purl.obolibrary.org/obo/GAZ_00236867 -->

    <owl:NamedIndividual rdf:about="http://purl.obolibrary.org/obo/GAZ_00236867">
        <obo:RO_0001025 rdf:resource="http://purl.obolibrary.org/obo/GAZ_00015419"/>
        <obo:IAO_0000115>A fourth-level administrative division of Uganda.</obo:IAO_0000115>
        <oboInOwl:hasOBONamespace>GAZ</oboInOwl:hasOBONamespace>
        <oboInOwl:id>GAZ:00236867</oboInOwl:id>
        <rdfs:label>Pingire Sub-count</rdfs:label>
    </owl:NamedIndividual>
    


    <!-- http://purl.obolibrary.org/obo/GAZ_00236868 -->

    <owl:NamedIndividual rdf:about="http://purl.obolibrary.org/obo/GAZ_00236868">
        <obo:RO_0001025 rdf:resource="http://purl.obolibrary.org/obo/GAZ_00015417"/>
        <obo:IAO_0000115>A fourth-level administrative division of Uganda.</obo:IAO_0000115>
        <oboInOwl:hasOBONamespace>GAZ</oboInOwl:hasOBONamespace>
        <oboInOwl:id>GAZ:00236868</oboInOwl:id>
        <rdfs:label>Atiira Sub-county</rdfs:label>
    </owl:NamedIndividual>
    


    <!-- http://purl.obolibrary.org/obo/GAZ_00236869 -->

    <owl:NamedIndividual rdf:about="http://purl.obolibrary.org/obo/GAZ_00236869">
        <obo:RO_0001025 rdf:resource="http://purl.obolibrary.org/obo/GAZ_00015417"/>
        <obo:IAO_0000115>A fourth-level administrative division of Uganda.</obo:IAO_0000115>
        <oboInOwl:hasOBONamespace>GAZ</oboInOwl:hasOBONamespace>
        <oboInOwl:id>GAZ:00236869</oboInOwl:id>
        <rdfs:label>Kateta Sub-county</rdfs:label>
    </owl:NamedIndividual>
    


    <!-- http://purl.obolibrary.org/obo/GAZ_00236870 -->

    <owl:NamedIndividual rdf:about="http://purl.obolibrary.org/obo/GAZ_00236870">
        <obo:RO_0001025 rdf:resource="http://purl.obolibrary.org/obo/GAZ_00015417"/>
        <obo:IAO_0000115>A fourth-level administrative division of Uganda.</obo:IAO_0000115>
        <oboInOwl:hasOBONamespace>GAZ</oboInOwl:hasOBONamespace>
        <oboInOwl:id>GAZ:00236870</oboInOwl:id>
        <rdfs:label>Kyere Sub-county</rdfs:label>
    </owl:NamedIndividual>
    


    <!-- http://purl.obolibrary.org/obo/GAZ_00236871 -->

    <owl:NamedIndividual rdf:about="http://purl.obolibrary.org/obo/GAZ_00236871">
        <obo:RO_0001025 rdf:resource="http://purl.obolibrary.org/obo/GAZ_00015417"/>
        <obo:IAO_0000115>A fourth-level administrative division of Uganda.</obo:IAO_0000115>
        <oboInOwl:hasOBONamespace>GAZ</oboInOwl:hasOBONamespace>
        <oboInOwl:id>GAZ:00236871</oboInOwl:id>
        <rdfs:label>Olio Sub-county</rdfs:label>
    </owl:NamedIndividual>
    


    <!-- http://purl.obolibrary.org/obo/GAZ_00236872 -->

    <owl:NamedIndividual rdf:about="http://purl.obolibrary.org/obo/GAZ_00236872">
        <obo:RO_0001025 rdf:resource="http://purl.obolibrary.org/obo/GAZ_00015418"/>
        <obo:IAO_0000115>A fourth-level administrative division of Uganda.</obo:IAO_0000115>
        <oboInOwl:hasOBONamespace>GAZ</oboInOwl:hasOBONamespace>
        <oboInOwl:id>GAZ:00236872</oboInOwl:id>
        <rdfs:label>Arapaix Sub-county</rdfs:label>
    </owl:NamedIndividual>
    


    <!-- http://purl.obolibrary.org/obo/GAZ_00236873 -->

    <owl:NamedIndividual rdf:about="http://purl.obolibrary.org/obo/GAZ_00236873">
        <obo:RO_0001025 rdf:resource="http://purl.obolibrary.org/obo/GAZ_00015418"/>
        <obo:IAO_0000115>A fourth-level administrative division of Uganda.</obo:IAO_0000115>
        <oboInOwl:hasOBONamespace>GAZ</oboInOwl:hasOBONamespace>
        <oboInOwl:id>GAZ:00236873</oboInOwl:id>
        <rdfs:label>Asuret Sub-county</rdfs:label>
    </owl:NamedIndividual>
    


    <!-- http://purl.obolibrary.org/obo/GAZ_00236874 -->

    <owl:NamedIndividual rdf:about="http://purl.obolibrary.org/obo/GAZ_00236874">
        <obo:RO_0001025 rdf:resource="http://purl.obolibrary.org/obo/GAZ_00015418"/>
        <obo:IAO_0000115>A fourth-level administrative division of Uganda.</obo:IAO_0000115>
        <oboInOwl:hasOBONamespace>GAZ</oboInOwl:hasOBONamespace>
        <oboInOwl:id>GAZ:00236874</oboInOwl:id>
        <rdfs:label>Gweri Sub-county</rdfs:label>
    </owl:NamedIndividual>
    


    <!-- http://purl.obolibrary.org/obo/GAZ_00236875 -->

    <owl:NamedIndividual rdf:about="http://purl.obolibrary.org/obo/GAZ_00236875">
        <obo:RO_0001025 rdf:resource="http://purl.obolibrary.org/obo/GAZ_00015418"/>
        <obo:IAO_0000115>A fourth-level administrative division of Uganda.</obo:IAO_0000115>
        <oboInOwl:hasOBONamespace>GAZ</oboInOwl:hasOBONamespace>
        <oboInOwl:id>GAZ:00236875</oboInOwl:id>
        <rdfs:label>Kamuda Sub-county</rdfs:label>
    </owl:NamedIndividual>
    


    <!-- http://purl.obolibrary.org/obo/GAZ_00236876 -->

    <owl:NamedIndividual rdf:about="http://purl.obolibrary.org/obo/GAZ_00236876">
        <obo:RO_0001025 rdf:resource="http://purl.obolibrary.org/obo/GAZ_00015418"/>
        <obo:IAO_0000115>A fourth-level administrative division of Uganda.</obo:IAO_0000115>
        <oboInOwl:hasOBONamespace>GAZ</oboInOwl:hasOBONamespace>
        <oboInOwl:id>GAZ:00236876</oboInOwl:id>
        <rdfs:label>Katine Sub-county</rdfs:label>
    </owl:NamedIndividual>
    


    <!-- http://purl.obolibrary.org/obo/GAZ_00236877 -->

    <owl:NamedIndividual rdf:about="http://purl.obolibrary.org/obo/GAZ_00236877">
        <obo:RO_0001025 rdf:resource="http://purl.obolibrary.org/obo/GAZ_00015418"/>
        <obo:IAO_0000115>A fourth-level administrative division of Uganda.</obo:IAO_0000115>
        <oboInOwl:hasOBONamespace>GAZ</oboInOwl:hasOBONamespace>
        <oboInOwl:id>GAZ:00236877</oboInOwl:id>
        <rdfs:label>Soroti Sub-county</rdfs:label>
    </owl:NamedIndividual>
    


    <!-- http://purl.obolibrary.org/obo/GAZ_00236878 -->

    <owl:NamedIndividual rdf:about="http://purl.obolibrary.org/obo/GAZ_00236878">
        <obo:RO_0001025 rdf:resource="http://purl.obolibrary.org/obo/GAZ_00015418"/>
        <obo:IAO_0000115>A fourth-level administrative division of Uganda.</obo:IAO_0000115>
        <oboInOwl:hasOBONamespace>GAZ</oboInOwl:hasOBONamespace>
        <oboInOwl:id>GAZ:00236878</oboInOwl:id>
        <rdfs:label>Tubur Sub-county</rdfs:label>
    </owl:NamedIndividual>
    


    <!-- http://purl.obolibrary.org/obo/GAZ_00236879 -->

    <owl:NamedIndividual rdf:about="http://purl.obolibrary.org/obo/GAZ_00236879">
        <obo:RO_0001025 rdf:resource="http://purl.obolibrary.org/obo/GAZ_00015418"/>
        <obo:IAO_0000115>A fourth-level administrative division of Uganda.</obo:IAO_0000115>
        <oboInOwl:hasOBONamespace>GAZ</oboInOwl:hasOBONamespace>
        <oboInOwl:id>GAZ:00236879</oboInOwl:id>
        <rdfs:label>Soroti Sub-county</rdfs:label>
    </owl:NamedIndividual>
    


    <!-- http://purl.obolibrary.org/obo/GAZ_00236880 -->

    <owl:NamedIndividual rdf:about="http://purl.obolibrary.org/obo/GAZ_00236880">
        <obo:RO_0001025 rdf:resource="http://purl.obolibrary.org/obo/GAZ_00015372"/>
        <obo:IAO_0000115>A fourth-level administrative division of Uganda.</obo:IAO_0000115>
        <oboInOwl:hasOBONamespace>GAZ</oboInOwl:hasOBONamespace>
        <oboInOwl:id>GAZ:00236880</oboInOwl:id>
        <rdfs:label>Municipality of Soroti</rdfs:label>
    </owl:NamedIndividual>
    


    <!-- http://purl.obolibrary.org/obo/GAZ_00236881 -->

    <owl:NamedIndividual rdf:about="http://purl.obolibrary.org/obo/GAZ_00236881">
        <obo:RO_0001025 rdf:resource="http://purl.obolibrary.org/obo/GAZ_00236880"/>
        <obo:IAO_0000115>A fourth-level administrative division of Uganda.</obo:IAO_0000115>
        <oboInOwl:hasOBONamespace>GAZ</oboInOwl:hasOBONamespace>
        <oboInOwl:id>GAZ:00236881</oboInOwl:id>
        <rdfs:label>Soroti Eastern Division</rdfs:label>
    </owl:NamedIndividual>
    


    <!-- http://purl.obolibrary.org/obo/GAZ_00236882 -->

    <owl:NamedIndividual rdf:about="http://purl.obolibrary.org/obo/GAZ_00236882">
        <obo:RO_0001025 rdf:resource="http://purl.obolibrary.org/obo/GAZ_00236880"/>
        <obo:IAO_0000115>A fourth-level administrative division of Uganda.</obo:IAO_0000115>
        <oboInOwl:hasOBONamespace>GAZ</oboInOwl:hasOBONamespace>
        <oboInOwl:id>GAZ:00236882</oboInOwl:id>
        <rdfs:label>Soroti Northern Division</rdfs:label>
    </owl:NamedIndividual>
    


    <!-- http://purl.obolibrary.org/obo/GAZ_00236883 -->

    <owl:NamedIndividual rdf:about="http://purl.obolibrary.org/obo/GAZ_00236883">
        <obo:RO_0001025 rdf:resource="http://purl.obolibrary.org/obo/GAZ_00236880"/>
        <obo:IAO_0000115>A fourth-level administrative division of Uganda.</obo:IAO_0000115>
        <oboInOwl:hasOBONamespace>GAZ</oboInOwl:hasOBONamespace>
        <oboInOwl:id>GAZ:00236883</oboInOwl:id>
        <rdfs:label>Soroti Western Division</rdfs:label>
    </owl:NamedIndividual>
    


    <!-- http://purl.obolibrary.org/obo/GAZ_00236884 -->

    <owl:NamedIndividual rdf:about="http://purl.obolibrary.org/obo/GAZ_00236884">
        <obo:RO_0001025 rdf:resource="http://purl.obolibrary.org/obo/GAZ_00015416"/>
        <obo:IAO_0000115>A fourth-level administrative division of Uganda.</obo:IAO_0000115>
        <oboInOwl:hasOBONamespace>GAZ</oboInOwl:hasOBONamespace>
        <oboInOwl:id>GAZ:00236884</oboInOwl:id>
        <rdfs:label>Iyolwa Sub-county</rdfs:label>
    </owl:NamedIndividual>
    


    <!-- http://purl.obolibrary.org/obo/GAZ_00236885 -->

    <owl:NamedIndividual rdf:about="http://purl.obolibrary.org/obo/GAZ_00236885">
        <obo:RO_0001025 rdf:resource="http://purl.obolibrary.org/obo/GAZ_00015416"/>
        <obo:IAO_0000115>A fourth-level administrative division of Uganda.</obo:IAO_0000115>
        <oboInOwl:hasOBONamespace>GAZ</oboInOwl:hasOBONamespace>
        <oboInOwl:id>GAZ:00236885</oboInOwl:id>
        <rdfs:label>Kirewa Sub-county</rdfs:label>
    </owl:NamedIndividual>
    


    <!-- http://purl.obolibrary.org/obo/GAZ_00236886 -->

    <owl:NamedIndividual rdf:about="http://purl.obolibrary.org/obo/GAZ_00236886">
        <obo:RO_0001025 rdf:resource="http://purl.obolibrary.org/obo/GAZ_00015416"/>
        <obo:IAO_0000115>A fourth-level administrative division of Uganda.</obo:IAO_0000115>
        <oboInOwl:hasOBONamespace>GAZ</oboInOwl:hasOBONamespace>
        <oboInOwl:id>GAZ:00236886</oboInOwl:id>
        <rdfs:label>Kisoko Sub-county</rdfs:label>
    </owl:NamedIndividual>
    


    <!-- http://purl.obolibrary.org/obo/GAZ_00236887 -->

    <owl:NamedIndividual rdf:about="http://purl.obolibrary.org/obo/GAZ_00236887">
        <obo:RO_0001025 rdf:resource="http://purl.obolibrary.org/obo/GAZ_00015416"/>
        <obo:IAO_0000115>A fourth-level administrative division of Uganda.</obo:IAO_0000115>
        <oboInOwl:hasOBONamespace>GAZ</oboInOwl:hasOBONamespace>
        <oboInOwl:id>GAZ:00236887</oboInOwl:id>
        <rdfs:label>Mulanda Sub-county</rdfs:label>
    </owl:NamedIndividual>
    


    <!-- http://purl.obolibrary.org/obo/GAZ_00236888 -->

    <owl:NamedIndividual rdf:about="http://purl.obolibrary.org/obo/GAZ_00236888">
        <obo:RO_0001025 rdf:resource="http://purl.obolibrary.org/obo/GAZ_00015416"/>
        <obo:IAO_0000115>A fourth-level administrative division of Uganda.</obo:IAO_0000115>
        <oboInOwl:hasOBONamespace>GAZ</oboInOwl:hasOBONamespace>
        <oboInOwl:id>GAZ:00236888</oboInOwl:id>
        <rdfs:label>Nabuyoga Sub-county</rdfs:label>
    </owl:NamedIndividual>
    


    <!-- http://purl.obolibrary.org/obo/GAZ_00236889 -->

    <owl:NamedIndividual rdf:about="http://purl.obolibrary.org/obo/GAZ_00236889">
        <obo:RO_0001025 rdf:resource="http://purl.obolibrary.org/obo/GAZ_00015416"/>
        <obo:IAO_0000115>A fourth-level administrative division of Uganda.</obo:IAO_0000115>
        <oboInOwl:hasOBONamespace>GAZ</oboInOwl:hasOBONamespace>
        <oboInOwl:id>GAZ:00236889</oboInOwl:id>
        <rdfs:label>Nagongera Sub-county</rdfs:label>
    </owl:NamedIndividual>
    


    <!-- http://purl.obolibrary.org/obo/GAZ_00236890 -->

    <owl:NamedIndividual rdf:about="http://purl.obolibrary.org/obo/GAZ_00236890">
        <obo:RO_0001025 rdf:resource="http://purl.obolibrary.org/obo/GAZ_00015416"/>
        <obo:IAO_0000115>A fourth-level administrative division of Uganda.</obo:IAO_0000115>
        <oboInOwl:hasOBONamespace>GAZ</oboInOwl:hasOBONamespace>
        <oboInOwl:id>GAZ:00236890</oboInOwl:id>
        <rdfs:label>Paya Sub-county</rdfs:label>
    </owl:NamedIndividual>
    


    <!-- http://purl.obolibrary.org/obo/GAZ_00236891 -->

    <owl:NamedIndividual rdf:about="http://purl.obolibrary.org/obo/GAZ_00236891">
        <obo:RO_0001025 rdf:resource="http://purl.obolibrary.org/obo/GAZ_00015416"/>
        <obo:IAO_0000115>A fourth-level administrative division of Uganda.</obo:IAO_0000115>
        <oboInOwl:hasOBONamespace>GAZ</oboInOwl:hasOBONamespace>
        <oboInOwl:id>GAZ:00236891</oboInOwl:id>
        <rdfs:label>Petta Sub-county</rdfs:label>
    </owl:NamedIndividual>
    


    <!-- http://purl.obolibrary.org/obo/GAZ_00236892 -->

    <owl:NamedIndividual rdf:about="http://purl.obolibrary.org/obo/GAZ_00236892">
        <obo:RO_0001025 rdf:resource="http://purl.obolibrary.org/obo/GAZ_00015416"/>
        <obo:IAO_0000115>A fourth-level administrative division of Uganda.</obo:IAO_0000115>
        <oboInOwl:hasOBONamespace>GAZ</oboInOwl:hasOBONamespace>
        <oboInOwl:id>GAZ:00236892</oboInOwl:id>
        <rdfs:label>Rubongi Sub-county</rdfs:label>
    </owl:NamedIndividual>
    


    <!-- http://purl.obolibrary.org/obo/GAZ_00236893 -->

    <owl:NamedIndividual rdf:about="http://purl.obolibrary.org/obo/GAZ_00236893">
        <obo:RO_0001025 rdf:resource="http://purl.obolibrary.org/obo/GAZ_00015415"/>
        <obo:IAO_0000115>A fourth-level administrative division of Uganda.</obo:IAO_0000115>
        <oboInOwl:hasOBONamespace>GAZ</oboInOwl:hasOBONamespace>
        <oboInOwl:id>GAZ:00236893</oboInOwl:id>
        <rdfs:label>Kwapa Sub-county</rdfs:label>
    </owl:NamedIndividual>
    


    <!-- http://purl.obolibrary.org/obo/GAZ_00236894 -->

    <owl:NamedIndividual rdf:about="http://purl.obolibrary.org/obo/GAZ_00236894">
        <obo:RO_0001025 rdf:resource="http://purl.obolibrary.org/obo/GAZ_00015415"/>
        <obo:IAO_0000115>A fourth-level administrative division of Uganda.</obo:IAO_0000115>
        <oboInOwl:hasOBONamespace>GAZ</oboInOwl:hasOBONamespace>
        <oboInOwl:id>GAZ:00236894</oboInOwl:id>
        <rdfs:label>Mella Sub-county</rdfs:label>
    </owl:NamedIndividual>
    


    <!-- http://purl.obolibrary.org/obo/GAZ_00236895 -->

    <owl:NamedIndividual rdf:about="http://purl.obolibrary.org/obo/GAZ_00236895">
        <obo:RO_0001025 rdf:resource="http://purl.obolibrary.org/obo/GAZ_00015415"/>
        <obo:IAO_0000115>A fourth-level administrative division of Uganda.</obo:IAO_0000115>
        <oboInOwl:hasOBONamespace>GAZ</oboInOwl:hasOBONamespace>
        <oboInOwl:id>GAZ:00236895</oboInOwl:id>
        <rdfs:label>Merikit Sub-county</rdfs:label>
    </owl:NamedIndividual>
    


    <!-- http://purl.obolibrary.org/obo/GAZ_00236896 -->

    <owl:NamedIndividual rdf:about="http://purl.obolibrary.org/obo/GAZ_00236896">
        <obo:RO_0001025 rdf:resource="http://purl.obolibrary.org/obo/GAZ_00015415"/>
        <obo:IAO_0000115>A fourth-level administrative division of Uganda.</obo:IAO_0000115>
        <oboInOwl:hasOBONamespace>GAZ</oboInOwl:hasOBONamespace>
        <oboInOwl:id>GAZ:00236896</oboInOwl:id>
        <rdfs:label>Molo Sub-county</rdfs:label>
    </owl:NamedIndividual>
    


    <!-- http://purl.obolibrary.org/obo/GAZ_00236897 -->

    <owl:NamedIndividual rdf:about="http://purl.obolibrary.org/obo/GAZ_00236897">
        <obo:RO_0001025 rdf:resource="http://purl.obolibrary.org/obo/GAZ_00015415"/>
        <obo:IAO_0000115>A fourth-level administrative division of Uganda.</obo:IAO_0000115>
        <oboInOwl:hasOBONamespace>GAZ</oboInOwl:hasOBONamespace>
        <oboInOwl:id>GAZ:00236897</oboInOwl:id>
        <rdfs:label>Mukuju Sub-county</rdfs:label>
    </owl:NamedIndividual>
    


    <!-- http://purl.obolibrary.org/obo/GAZ_00236898 -->

    <owl:NamedIndividual rdf:about="http://purl.obolibrary.org/obo/GAZ_00236898">
        <obo:RO_0001025 rdf:resource="http://purl.obolibrary.org/obo/GAZ_00015415"/>
        <obo:IAO_0000115>A fourth-level administrative division of Uganda.</obo:IAO_0000115>
        <oboInOwl:hasOBONamespace>GAZ</oboInOwl:hasOBONamespace>
        <oboInOwl:id>GAZ:00236898</oboInOwl:id>
        <rdfs:label>Osukuru Sub-county</rdfs:label>
    </owl:NamedIndividual>
    


    <!-- http://purl.obolibrary.org/obo/GAZ_00236899 -->

    <owl:NamedIndividual rdf:about="http://purl.obolibrary.org/obo/GAZ_00236899">
        <obo:RO_0001025 rdf:resource="http://purl.obolibrary.org/obo/GAZ_00015371"/>
        <obo:IAO_0000115>A fourth-level administrative division of Uganda.</obo:IAO_0000115>
        <oboInOwl:hasOBONamespace>GAZ</oboInOwl:hasOBONamespace>
        <oboInOwl:id>GAZ:00236899</oboInOwl:id>
        <rdfs:label>Municipality of Tororo</rdfs:label>
    </owl:NamedIndividual>
    


    <!-- http://purl.obolibrary.org/obo/GAZ_00236900 -->

    <owl:NamedIndividual rdf:about="http://purl.obolibrary.org/obo/GAZ_00236900">
        <obo:RO_0001025 rdf:resource="http://purl.obolibrary.org/obo/GAZ_00236899"/>
        <obo:IAO_0000115>A fourth-level administrative division of Uganda.</obo:IAO_0000115>
        <oboInOwl:hasOBONamespace>GAZ</oboInOwl:hasOBONamespace>
        <oboInOwl:id>GAZ:00236900</oboInOwl:id>
        <rdfs:label>Tororo Eastern Division</rdfs:label>
    </owl:NamedIndividual>
    


    <!-- http://purl.obolibrary.org/obo/GAZ_00236901 -->

    <owl:NamedIndividual rdf:about="http://purl.obolibrary.org/obo/GAZ_00236901">
        <obo:RO_0001025 rdf:resource="http://purl.obolibrary.org/obo/GAZ_00236899"/>
        <obo:IAO_0000115>A fourth-level administrative division of Uganda.</obo:IAO_0000115>
        <oboInOwl:hasOBONamespace>GAZ</oboInOwl:hasOBONamespace>
        <oboInOwl:id>GAZ:00236901</oboInOwl:id>
        <rdfs:label>Tororo Western Division</rdfs:label>
    </owl:NamedIndividual>
    


    <!-- http://purl.obolibrary.org/obo/GAZ_00236902 -->

    <owl:NamedIndividual rdf:about="http://purl.obolibrary.org/obo/GAZ_00236902">
        <obo:IAO_0000115>A fourth-level administrative division of Uganda.</obo:IAO_0000115>
        <oboInOwl:hasOBONamespace>GAZ</oboInOwl:hasOBONamespace>
        <oboInOwl:id>GAZ:00236902</oboInOwl:id>
        <rdfs:label>Abim Sub-county</rdfs:label>
    </owl:NamedIndividual>
    


    <!-- http://purl.obolibrary.org/obo/GAZ_00236903 -->

    <owl:NamedIndividual rdf:about="http://purl.obolibrary.org/obo/GAZ_00236903">
        <obo:IAO_0000115>A fourth-level administrative division of Uganda.</obo:IAO_0000115>
        <oboInOwl:hasOBONamespace>GAZ</oboInOwl:hasOBONamespace>
        <oboInOwl:id>GAZ:00236903</oboInOwl:id>
        <rdfs:label>Alerek Sub-county</rdfs:label>
    </owl:NamedIndividual>
    


    <!-- http://purl.obolibrary.org/obo/GAZ_00236904 -->

    <owl:NamedIndividual rdf:about="http://purl.obolibrary.org/obo/GAZ_00236904">
        <obo:IAO_0000115>A fourth-level administrative division of Uganda.</obo:IAO_0000115>
        <oboInOwl:hasOBONamespace>GAZ</oboInOwl:hasOBONamespace>
        <oboInOwl:id>GAZ:00236904</oboInOwl:id>
        <rdfs:label>Lotukei Sub-county</rdfs:label>
    </owl:NamedIndividual>
    


    <!-- http://purl.obolibrary.org/obo/GAZ_00236905 -->

    <owl:NamedIndividual rdf:about="http://purl.obolibrary.org/obo/GAZ_00236905">
        <obo:IAO_0000115>A fourth-level administrative division of Uganda.</obo:IAO_0000115>
        <oboInOwl:hasOBONamespace>GAZ</oboInOwl:hasOBONamespace>
        <oboInOwl:id>GAZ:00236905</oboInOwl:id>
        <rdfs:label>Morulem Sub-county</rdfs:label>
    </owl:NamedIndividual>
    


    <!-- http://purl.obolibrary.org/obo/GAZ_00236906 -->

    <owl:NamedIndividual rdf:about="http://purl.obolibrary.org/obo/GAZ_00236906">
        <obo:IAO_0000115>A fourth-level administrative division of Uganda.</obo:IAO_0000115>
        <oboInOwl:hasOBONamespace>GAZ</oboInOwl:hasOBONamespace>
        <oboInOwl:id>GAZ:00236906</oboInOwl:id>
        <rdfs:label>Nyakwae Sub-county</rdfs:label>
    </owl:NamedIndividual>
    


    <!-- http://purl.obolibrary.org/obo/GAZ_00236907 -->

    <owl:NamedIndividual rdf:about="http://purl.obolibrary.org/obo/GAZ_00236907">
        <obo:RO_0001025 rdf:resource="http://purl.obolibrary.org/obo/GAZ_00015485"/>
        <obo:IAO_0000115>A fourth-level administrative division of Uganda.</obo:IAO_0000115>
        <oboInOwl:hasOBONamespace>GAZ</oboInOwl:hasOBONamespace>
        <oboInOwl:id>GAZ:00236907</oboInOwl:id>
        <rdfs:label>Adjumani Town</rdfs:label>
    </owl:NamedIndividual>
    


    <!-- http://purl.obolibrary.org/obo/GAZ_00236908 -->

    <owl:NamedIndividual rdf:about="http://purl.obolibrary.org/obo/GAZ_00236908">
        <obo:RO_0001025 rdf:resource="http://purl.obolibrary.org/obo/GAZ_00015485"/>
        <obo:IAO_0000115>A fourth-level administrative division of Uganda.</obo:IAO_0000115>
        <oboInOwl:hasOBONamespace>GAZ</oboInOwl:hasOBONamespace>
        <oboInOwl:id>GAZ:00236908</oboInOwl:id>
        <rdfs:label>Adropi Sub-county</rdfs:label>
    </owl:NamedIndividual>
    


    <!-- http://purl.obolibrary.org/obo/GAZ_00236909 -->

    <owl:NamedIndividual rdf:about="http://purl.obolibrary.org/obo/GAZ_00236909">
        <obo:RO_0001025 rdf:resource="http://purl.obolibrary.org/obo/GAZ_00015485"/>
        <obo:IAO_0000115>A fourth-level administrative division of Uganda.</obo:IAO_0000115>
        <oboInOwl:hasOBONamespace>GAZ</oboInOwl:hasOBONamespace>
        <oboInOwl:id>GAZ:00236909</oboInOwl:id>
        <rdfs:label>Ciforo Sub-county</rdfs:label>
    </owl:NamedIndividual>
    


    <!-- http://purl.obolibrary.org/obo/GAZ_00236910 -->

    <owl:NamedIndividual rdf:about="http://purl.obolibrary.org/obo/GAZ_00236910">
        <obo:RO_0001025 rdf:resource="http://purl.obolibrary.org/obo/GAZ_00015485"/>
        <obo:IAO_0000115>A fourth-level administrative division of Uganda.</obo:IAO_0000115>
        <oboInOwl:hasOBONamespace>GAZ</oboInOwl:hasOBONamespace>
        <oboInOwl:id>GAZ:00236910</oboInOwl:id>
        <rdfs:label>Dzaipi Sub-county</rdfs:label>
    </owl:NamedIndividual>
    


    <!-- http://purl.obolibrary.org/obo/GAZ_00236911 -->

    <owl:NamedIndividual rdf:about="http://purl.obolibrary.org/obo/GAZ_00236911">
        <obo:RO_0001025 rdf:resource="http://purl.obolibrary.org/obo/GAZ_00015485"/>
        <obo:IAO_0000115>A fourth-level administrative division of Uganda.</obo:IAO_0000115>
        <oboInOwl:hasOBONamespace>GAZ</oboInOwl:hasOBONamespace>
        <oboInOwl:id>GAZ:00236911</oboInOwl:id>
        <rdfs:label>Ofua Sub-county</rdfs:label>
    </owl:NamedIndividual>
    


    <!-- http://purl.obolibrary.org/obo/GAZ_00236912 -->

    <owl:NamedIndividual rdf:about="http://purl.obolibrary.org/obo/GAZ_00236912">
        <obo:RO_0001025 rdf:resource="http://purl.obolibrary.org/obo/GAZ_00015485"/>
        <obo:IAO_0000115>A fourth-level administrative division of Uganda.</obo:IAO_0000115>
        <oboInOwl:hasOBONamespace>GAZ</oboInOwl:hasOBONamespace>
        <oboInOwl:id>GAZ:00236912</oboInOwl:id>
        <rdfs:label>Pakelle Sub-county</rdfs:label>
    </owl:NamedIndividual>
    


    <!-- http://purl.obolibrary.org/obo/GAZ_00236913 -->

    <owl:NamedIndividual rdf:about="http://purl.obolibrary.org/obo/GAZ_00236913">
        <obo:RO_0001025 rdf:resource="http://purl.obolibrary.org/obo/GAZ_00015486"/>
        <obo:IAO_0000115>A fourth-level administrative division of Uganda.</obo:IAO_0000115>
        <oboInOwl:hasOBONamespace>GAZ</oboInOwl:hasOBONamespace>
        <oboInOwl:id>GAZ:00236913</oboInOwl:id>
        <rdfs:label>Aputi Sub-county</rdfs:label>
    </owl:NamedIndividual>
    


    <!-- http://purl.obolibrary.org/obo/GAZ_00236914 -->

    <owl:NamedIndividual rdf:about="http://purl.obolibrary.org/obo/GAZ_00236914">
        <obo:RO_0001025 rdf:resource="http://purl.obolibrary.org/obo/GAZ_00015486"/>
        <obo:IAO_0000115>A fourth-level administrative division of Uganda.</obo:IAO_0000115>
        <oboInOwl:hasOBONamespace>GAZ</oboInOwl:hasOBONamespace>
        <oboInOwl:id>GAZ:00236914</oboInOwl:id>
        <rdfs:label>Awelo Sub-county</rdfs:label>
    </owl:NamedIndividual>
    


    <!-- http://purl.obolibrary.org/obo/GAZ_00236915 -->

    <owl:NamedIndividual rdf:about="http://purl.obolibrary.org/obo/GAZ_00236915">
        <obo:RO_0001025 rdf:resource="http://purl.obolibrary.org/obo/GAZ_00015486"/>
        <obo:IAO_0000115>A fourth-level administrative division of Uganda.</obo:IAO_0000115>
        <oboInOwl:hasOBONamespace>GAZ</oboInOwl:hasOBONamespace>
        <oboInOwl:id>GAZ:00236915</oboInOwl:id>
        <rdfs:label>Muntu Sub-county</rdfs:label>
    </owl:NamedIndividual>
    


    <!-- http://purl.obolibrary.org/obo/GAZ_00236916 -->

    <owl:NamedIndividual rdf:about="http://purl.obolibrary.org/obo/GAZ_00236916">
        <obo:RO_0001025 rdf:resource="http://purl.obolibrary.org/obo/GAZ_00015486"/>
        <obo:IAO_0000115>A fourth-level administrative division of Uganda.</obo:IAO_0000115>
        <oboInOwl:hasOBONamespace>GAZ</oboInOwl:hasOBONamespace>
        <oboInOwl:id>GAZ:00236916</oboInOwl:id>
        <rdfs:label>Namasale Sub-county</rdfs:label>
    </owl:NamedIndividual>
    


    <!-- http://purl.obolibrary.org/obo/GAZ_00236917 -->

    <owl:NamedIndividual rdf:about="http://purl.obolibrary.org/obo/GAZ_00236917">
        <obo:RO_0001025 rdf:resource="http://purl.obolibrary.org/obo/GAZ_00005375"/>
        <obo:IAO_0000115>A subregion of the Northern Region of Uganda.</obo:IAO_0000115>
        <oboInOwl:hasOBONamespace>GAZ</oboInOwl:hasOBONamespace>
        <oboInOwl:id>GAZ:00236917</oboInOwl:id>
        <rdfs:label>Acholi Subregion</rdfs:label>
    </owl:NamedIndividual>
    


    <!-- http://purl.obolibrary.org/obo/GAZ_00236918 -->

    <owl:NamedIndividual rdf:about="http://purl.obolibrary.org/obo/GAZ_00236918">
        <obo:RO_0001025 rdf:resource="http://purl.obolibrary.org/obo/GAZ_00015487"/>
        <obo:IAO_0000115>A fourth-level administrative division of Uganda.</obo:IAO_0000115>
        <oboInOwl:hasOBONamespace>GAZ</oboInOwl:hasOBONamespace>
        <oboInOwl:id>GAZ:00236918</oboInOwl:id>
        <rdfs:label>Amuru Sub-county</rdfs:label>
    </owl:NamedIndividual>
    


    <!-- http://purl.obolibrary.org/obo/GAZ_00236919 -->

    <owl:NamedIndividual rdf:about="http://purl.obolibrary.org/obo/GAZ_00236919">
        <obo:RO_0001025 rdf:resource="http://purl.obolibrary.org/obo/GAZ_00015487"/>
        <obo:IAO_0000115>A fourth-level administrative division of Uganda.</obo:IAO_0000115>
        <oboInOwl:hasOBONamespace>GAZ</oboInOwl:hasOBONamespace>
        <oboInOwl:id>GAZ:00236919</oboInOwl:id>
        <rdfs:label>Atiak Sub-county</rdfs:label>
    </owl:NamedIndividual>
    


    <!-- http://purl.obolibrary.org/obo/GAZ_00236920 -->

    <owl:NamedIndividual rdf:about="http://purl.obolibrary.org/obo/GAZ_00236920">
        <obo:RO_0001025 rdf:resource="http://purl.obolibrary.org/obo/GAZ_00015487"/>
        <obo:IAO_0000115>A fourth-level administrative division of Uganda.</obo:IAO_0000115>
        <oboInOwl:hasOBONamespace>GAZ</oboInOwl:hasOBONamespace>
        <oboInOwl:id>GAZ:00236920</oboInOwl:id>
        <rdfs:label>Lamogi Sub-county</rdfs:label>
    </owl:NamedIndividual>
    


    <!-- http://purl.obolibrary.org/obo/GAZ_00236921 -->

    <owl:NamedIndividual rdf:about="http://purl.obolibrary.org/obo/GAZ_00236921">
        <obo:RO_0001025 rdf:resource="http://purl.obolibrary.org/obo/GAZ_00015487"/>
        <obo:IAO_0000115>A fourth-level administrative division of Uganda.</obo:IAO_0000115>
        <oboInOwl:hasOBONamespace>GAZ</oboInOwl:hasOBONamespace>
        <oboInOwl:id>GAZ:00236921</oboInOwl:id>
        <rdfs:label>Pabbo Sub-county</rdfs:label>
    </owl:NamedIndividual>
    


    <!-- http://purl.obolibrary.org/obo/GAZ_00236922 -->

    <owl:NamedIndividual rdf:about="http://purl.obolibrary.org/obo/GAZ_00236922">
        <obo:RO_0001025 rdf:resource="http://purl.obolibrary.org/obo/GAZ_00015488"/>
        <obo:IAO_0000115>A fourth-level administrative division of Uganda.</obo:IAO_0000115>
        <oboInOwl:hasOBONamespace>GAZ</oboInOwl:hasOBONamespace>
        <oboInOwl:id>GAZ:00236922</oboInOwl:id>
        <rdfs:label>Alero Sub-county</rdfs:label>
    </owl:NamedIndividual>
    


    <!-- http://purl.obolibrary.org/obo/GAZ_00236923 -->

    <owl:NamedIndividual rdf:about="http://purl.obolibrary.org/obo/GAZ_00236923">
        <obo:RO_0001025 rdf:resource="http://purl.obolibrary.org/obo/GAZ_00015488"/>
        <obo:IAO_0000115>A fourth-level administrative division of Uganda.</obo:IAO_0000115>
        <oboInOwl:hasOBONamespace>GAZ</oboInOwl:hasOBONamespace>
        <oboInOwl:id>GAZ:00236923</oboInOwl:id>
        <rdfs:label>Anaka Sub-county</rdfs:label>
    </owl:NamedIndividual>
    


    <!-- http://purl.obolibrary.org/obo/GAZ_00236924 -->

    <owl:NamedIndividual rdf:about="http://purl.obolibrary.org/obo/GAZ_00236924">
        <obo:RO_0001025 rdf:resource="http://purl.obolibrary.org/obo/GAZ_00015488"/>
        <obo:IAO_0000115>A fourth-level administrative division of Uganda.</obo:IAO_0000115>
        <oboInOwl:hasOBONamespace>GAZ</oboInOwl:hasOBONamespace>
        <oboInOwl:id>GAZ:00236924</oboInOwl:id>
        <rdfs:label>Purongo Sub-county</rdfs:label>
    </owl:NamedIndividual>
    


    <!-- http://purl.obolibrary.org/obo/GAZ_00236925 -->

    <owl:NamedIndividual rdf:about="http://purl.obolibrary.org/obo/GAZ_00236925">
        <obo:RO_0001025 rdf:resource="http://purl.obolibrary.org/obo/GAZ_00015488"/>
        <obo:IAO_0000115>A fourth-level administrative division of Uganda.</obo:IAO_0000115>
        <oboInOwl:hasOBONamespace>GAZ</oboInOwl:hasOBONamespace>
        <oboInOwl:id>GAZ:00236925</oboInOwl:id>
        <rdfs:label>Koch Goma Sub-county</rdfs:label>
    </owl:NamedIndividual>
    


    <!-- http://purl.obolibrary.org/obo/GAZ_00236926 -->

    <owl:NamedIndividual rdf:about="http://purl.obolibrary.org/obo/GAZ_00236926">
        <obo:RO_0001025 rdf:resource="http://purl.obolibrary.org/obo/GAZ_00015489"/>
        <obo:IAO_0000115>A fourth-level administrative division of Uganda.</obo:IAO_0000115>
        <oboInOwl:hasOBONamespace>GAZ</oboInOwl:hasOBONamespace>
        <oboInOwl:id>GAZ:00236926</oboInOwl:id>
        <rdfs:label>Aboke Sub-county</rdfs:label>
    </owl:NamedIndividual>
    


    <!-- http://purl.obolibrary.org/obo/GAZ_00236927 -->

    <owl:NamedIndividual rdf:about="http://purl.obolibrary.org/obo/GAZ_00236927">
        <obo:RO_0001025 rdf:resource="http://purl.obolibrary.org/obo/GAZ_00015489"/>
        <obo:IAO_0000115>A fourth-level administrative division of Uganda.</obo:IAO_0000115>
        <oboInOwl:hasOBONamespace>GAZ</oboInOwl:hasOBONamespace>
        <oboInOwl:id>GAZ:00236927</oboInOwl:id>
        <rdfs:label>Akalo Sub-county</rdfs:label>
    </owl:NamedIndividual>
    


    <!-- http://purl.obolibrary.org/obo/GAZ_00236928 -->

    <owl:NamedIndividual rdf:about="http://purl.obolibrary.org/obo/GAZ_00236928">
        <obo:RO_0001025 rdf:resource="http://purl.obolibrary.org/obo/GAZ_00015489"/>
        <obo:IAO_0000115>A fourth-level administrative division of Uganda.</obo:IAO_0000115>
        <oboInOwl:hasOBONamespace>GAZ</oboInOwl:hasOBONamespace>
        <oboInOwl:id>GAZ:00236928</oboInOwl:id>
        <rdfs:label>Alito Sub-county</rdfs:label>
    </owl:NamedIndividual>
    


    <!-- http://purl.obolibrary.org/obo/GAZ_00236929 -->

    <owl:NamedIndividual rdf:about="http://purl.obolibrary.org/obo/GAZ_00236929">
        <obo:RO_0001025 rdf:resource="http://purl.obolibrary.org/obo/GAZ_00015489"/>
        <obo:IAO_0000115>A fourth-level administrative division of Uganda.</obo:IAO_0000115>
        <oboInOwl:hasOBONamespace>GAZ</oboInOwl:hasOBONamespace>
        <oboInOwl:id>GAZ:00236929</oboInOwl:id>
        <rdfs:label>Ayer Sub-county</rdfs:label>
    </owl:NamedIndividual>
    


    <!-- http://purl.obolibrary.org/obo/GAZ_00236930 -->

    <owl:NamedIndividual rdf:about="http://purl.obolibrary.org/obo/GAZ_00236930">
        <obo:RO_0001025 rdf:resource="http://purl.obolibrary.org/obo/GAZ_00015489"/>
        <obo:IAO_0000115>A fourth-level administrative division of Uganda.</obo:IAO_0000115>
        <oboInOwl:hasOBONamespace>GAZ</oboInOwl:hasOBONamespace>
        <oboInOwl:id>GAZ:00236930</oboInOwl:id>
        <rdfs:label>Bala Sub-county</rdfs:label>
    </owl:NamedIndividual>
    


    <!-- http://purl.obolibrary.org/obo/GAZ_00236931 -->

    <owl:NamedIndividual rdf:about="http://purl.obolibrary.org/obo/GAZ_00236931">
        <obo:RO_0001025 rdf:resource="http://purl.obolibrary.org/obo/GAZ_00015490"/>
        <obo:IAO_0000115>A fourth-level administrative division of Uganda.</obo:IAO_0000115>
        <oboInOwl:hasOBONamespace>GAZ</oboInOwl:hasOBONamespace>
        <oboInOwl:id>GAZ:00236931</oboInOwl:id>
        <rdfs:label>Abongomola Sub-county</rdfs:label>
    </owl:NamedIndividual>
    


    <!-- http://purl.obolibrary.org/obo/GAZ_00236932 -->

    <owl:NamedIndividual rdf:about="http://purl.obolibrary.org/obo/GAZ_00236932">
        <obo:RO_0001025 rdf:resource="http://purl.obolibrary.org/obo/GAZ_00015490"/>
        <obo:IAO_0000115>A fourth-level administrative division of Uganda.</obo:IAO_0000115>
        <oboInOwl:hasOBONamespace>GAZ</oboInOwl:hasOBONamespace>
        <oboInOwl:id>GAZ:00236932</oboInOwl:id>
        <rdfs:label>Aduku Sub-county</rdfs:label>
    </owl:NamedIndividual>
    


    <!-- http://purl.obolibrary.org/obo/GAZ_00236933 -->

    <owl:NamedIndividual rdf:about="http://purl.obolibrary.org/obo/GAZ_00236933">
        <obo:RO_0001025 rdf:resource="http://purl.obolibrary.org/obo/GAZ_00015490"/>
        <obo:IAO_0000115>A fourth-level administrative division of Uganda.</obo:IAO_0000115>
        <oboInOwl:hasOBONamespace>GAZ</oboInOwl:hasOBONamespace>
        <oboInOwl:id>GAZ:00236933</oboInOwl:id>
        <rdfs:label>Chawente Sub-county</rdfs:label>
    </owl:NamedIndividual>
    


    <!-- http://purl.obolibrary.org/obo/GAZ_00236934 -->

    <owl:NamedIndividual rdf:about="http://purl.obolibrary.org/obo/GAZ_00236934">
        <obo:RO_0001025 rdf:resource="http://purl.obolibrary.org/obo/GAZ_00015490"/>
        <obo:IAO_0000115>A fourth-level administrative division of Uganda.</obo:IAO_0000115>
        <oboInOwl:hasOBONamespace>GAZ</oboInOwl:hasOBONamespace>
        <oboInOwl:id>GAZ:00236934</oboInOwl:id>
        <rdfs:label>Inomo Sub-county</rdfs:label>
    </owl:NamedIndividual>
    


    <!-- http://purl.obolibrary.org/obo/GAZ_00236935 -->

    <owl:NamedIndividual rdf:about="http://purl.obolibrary.org/obo/GAZ_00236935">
        <obo:RO_0001025 rdf:resource="http://purl.obolibrary.org/obo/GAZ_00015490"/>
        <obo:IAO_0000115>A fourth-level administrative division of Uganda.</obo:IAO_0000115>
        <oboInOwl:hasOBONamespace>GAZ</oboInOwl:hasOBONamespace>
        <oboInOwl:id>GAZ:00236935</oboInOwl:id>
        <rdfs:label>Nambieso Sub-county</rdfs:label>
    </owl:NamedIndividual>
    


    <!-- http://purl.obolibrary.org/obo/GAZ_00236936 -->

    <owl:NamedIndividual rdf:about="http://purl.obolibrary.org/obo/GAZ_00236936">
        <obo:RO_0001025 rdf:resource="http://purl.obolibrary.org/obo/GAZ_00015491"/>
        <obo:IAO_0000115>A fourth-level administrative division of Uganda.</obo:IAO_0000115>
        <oboInOwl:hasOBONamespace>GAZ</oboInOwl:hasOBONamespace>
        <oboInOwl:id>GAZ:00236936</oboInOwl:id>
        <rdfs:label>Akokoro Sub-county</rdfs:label>
    </owl:NamedIndividual>
    


    <!-- http://purl.obolibrary.org/obo/GAZ_00236937 -->

    <owl:NamedIndividual rdf:about="http://purl.obolibrary.org/obo/GAZ_00236937">
        <obo:RO_0001025 rdf:resource="http://purl.obolibrary.org/obo/GAZ_00015491"/>
        <obo:IAO_0000115>A fourth-level administrative division of Uganda.</obo:IAO_0000115>
        <oboInOwl:hasOBONamespace>GAZ</oboInOwl:hasOBONamespace>
        <oboInOwl:id>GAZ:00236937</oboInOwl:id>
        <rdfs:label>Apac Sub-county</rdfs:label>
    </owl:NamedIndividual>
    


    <!-- http://purl.obolibrary.org/obo/GAZ_00236938 -->

    <owl:NamedIndividual rdf:about="http://purl.obolibrary.org/obo/GAZ_00236938">
        <obo:RO_0001025 rdf:resource="http://purl.obolibrary.org/obo/GAZ_00015491"/>
        <obo:IAO_0000115>A fourth-level administrative division of Uganda.</obo:IAO_0000115>
        <oboInOwl:hasOBONamespace>GAZ</oboInOwl:hasOBONamespace>
        <oboInOwl:id>GAZ:00236938</oboInOwl:id>
        <rdfs:label>Apac Town</rdfs:label>
    </owl:NamedIndividual>
    


    <!-- http://purl.obolibrary.org/obo/GAZ_00236939 -->

    <owl:NamedIndividual rdf:about="http://purl.obolibrary.org/obo/GAZ_00236939">
        <obo:RO_0001025 rdf:resource="http://purl.obolibrary.org/obo/GAZ_00015491"/>
        <obo:IAO_0000115>A fourth-level administrative division of Uganda.</obo:IAO_0000115>
        <oboInOwl:hasOBONamespace>GAZ</oboInOwl:hasOBONamespace>
        <oboInOwl:id>GAZ:00236939</oboInOwl:id>
        <rdfs:label>Cegere Sub-county</rdfs:label>
    </owl:NamedIndividual>
    


    <!-- http://purl.obolibrary.org/obo/GAZ_00236940 -->

    <owl:NamedIndividual rdf:about="http://purl.obolibrary.org/obo/GAZ_00236940">
        <obo:RO_0001025 rdf:resource="http://purl.obolibrary.org/obo/GAZ_00015491"/>
        <obo:IAO_0000115>A fourth-level administrative division of Uganda.</obo:IAO_0000115>
        <oboInOwl:hasOBONamespace>GAZ</oboInOwl:hasOBONamespace>
        <oboInOwl:id>GAZ:00236940</oboInOwl:id>
        <rdfs:label>Ibuje Sub-county</rdfs:label>
    </owl:NamedIndividual>
    


    <!-- http://purl.obolibrary.org/obo/GAZ_00236941 -->

    <owl:NamedIndividual rdf:about="http://purl.obolibrary.org/obo/GAZ_00236941">
        <obo:RO_0001025 rdf:resource="http://purl.obolibrary.org/obo/GAZ_00015493"/>
        <obo:IAO_0000115>A fourth-level administrative division of Uganda.</obo:IAO_0000115>
        <oboInOwl:hasOBONamespace>GAZ</oboInOwl:hasOBONamespace>
        <oboInOwl:id>GAZ:00236941</oboInOwl:id>
        <rdfs:label>Arua Hill Sub-county</rdfs:label>
    </owl:NamedIndividual>
    


    <!-- http://purl.obolibrary.org/obo/GAZ_00236942 -->

    <owl:NamedIndividual rdf:about="http://purl.obolibrary.org/obo/GAZ_00236942">
        <obo:RO_0001025 rdf:resource="http://purl.obolibrary.org/obo/GAZ_00015493"/>
        <obo:IAO_0000115>A fourth-level administrative division of Uganda.</obo:IAO_0000115>
        <oboInOwl:hasOBONamespace>GAZ</oboInOwl:hasOBONamespace>
        <oboInOwl:id>GAZ:00236942</oboInOwl:id>
        <rdfs:label>Oli River Sub-county</rdfs:label>
    </owl:NamedIndividual>
    


    <!-- http://purl.obolibrary.org/obo/GAZ_00236943 -->

    <owl:NamedIndividual rdf:about="http://purl.obolibrary.org/obo/GAZ_00236943">
        <obo:RO_0001025 rdf:resource="http://purl.obolibrary.org/obo/GAZ_00015495"/>
        <obo:IAO_0000115>A fourth-level administrative division of Uganda.</obo:IAO_0000115>
        <oboInOwl:hasOBONamespace>GAZ</oboInOwl:hasOBONamespace>
        <oboInOwl:id>GAZ:00236943</oboInOwl:id>
        <rdfs:label>Adumi Sub-county</rdfs:label>
    </owl:NamedIndividual>
    


    <!-- http://purl.obolibrary.org/obo/GAZ_00236944 -->

    <owl:NamedIndividual rdf:about="http://purl.obolibrary.org/obo/GAZ_00236944">
        <obo:RO_0001025 rdf:resource="http://purl.obolibrary.org/obo/GAZ_00015495"/>
        <obo:IAO_0000115>A fourth-level administrative division of Uganda.</obo:IAO_0000115>
        <oboInOwl:hasOBONamespace>GAZ</oboInOwl:hasOBONamespace>
        <oboInOwl:id>GAZ:00236944</oboInOwl:id>
        <rdfs:label>Aroi Sub-county</rdfs:label>
    </owl:NamedIndividual>
    


    <!-- http://purl.obolibrary.org/obo/GAZ_00236945 -->

    <owl:NamedIndividual rdf:about="http://purl.obolibrary.org/obo/GAZ_00236945">
        <obo:RO_0001025 rdf:resource="http://purl.obolibrary.org/obo/GAZ_00015495"/>
        <obo:IAO_0000115>A fourth-level administrative division of Uganda.</obo:IAO_0000115>
        <oboInOwl:hasOBONamespace>GAZ</oboInOwl:hasOBONamespace>
        <oboInOwl:id>GAZ:00236945</oboInOwl:id>
        <rdfs:label>Dadamu Sub-county</rdfs:label>
    </owl:NamedIndividual>
    


    <!-- http://purl.obolibrary.org/obo/GAZ_00236946 -->

    <owl:NamedIndividual rdf:about="http://purl.obolibrary.org/obo/GAZ_00236946">
        <obo:RO_0001025 rdf:resource="http://purl.obolibrary.org/obo/GAZ_00015495"/>
        <obo:IAO_0000115>A fourth-level administrative division of Uganda.</obo:IAO_0000115>
        <oboInOwl:hasOBONamespace>GAZ</oboInOwl:hasOBONamespace>
        <oboInOwl:id>GAZ:00236946</oboInOwl:id>
        <rdfs:label>Manibe Sub-county</rdfs:label>
    </owl:NamedIndividual>
    


    <!-- http://purl.obolibrary.org/obo/GAZ_00236947 -->

    <owl:NamedIndividual rdf:about="http://purl.obolibrary.org/obo/GAZ_00236947">
        <obo:RO_0001025 rdf:resource="http://purl.obolibrary.org/obo/GAZ_00015495"/>
        <obo:IAO_0000115>A fourth-level administrative division of Uganda.</obo:IAO_0000115>
        <oboInOwl:hasOBONamespace>GAZ</oboInOwl:hasOBONamespace>
        <oboInOwl:id>GAZ:00236947</oboInOwl:id>
        <rdfs:label>Oluko Sub-county</rdfs:label>
    </owl:NamedIndividual>
    


    <!-- http://purl.obolibrary.org/obo/GAZ_00236948 -->

    <owl:NamedIndividual rdf:about="http://purl.obolibrary.org/obo/GAZ_00236948">
        <obo:RO_0001025 rdf:resource="http://purl.obolibrary.org/obo/GAZ_00015495"/>
        <obo:IAO_0000115>A fourth-level administrative division of Uganda.</obo:IAO_0000115>
        <oboInOwl:hasOBONamespace>GAZ</oboInOwl:hasOBONamespace>
        <oboInOwl:id>GAZ:00236948</oboInOwl:id>
        <rdfs:label>Pajulu Sub-county</rdfs:label>
    </owl:NamedIndividual>
    


    <!-- http://purl.obolibrary.org/obo/GAZ_00236949 -->

    <owl:NamedIndividual rdf:about="http://purl.obolibrary.org/obo/GAZ_00236949">
        <obo:IAO_0000115>A fourth-level administrative division of Uganda.</obo:IAO_0000115>
        <oboInOwl:hasOBONamespace>GAZ</oboInOwl:hasOBONamespace>
        <oboInOwl:id>GAZ:00236949</oboInOwl:id>
        <rdfs:label>Koboko Town</rdfs:label>
    </owl:NamedIndividual>
    


    <!-- http://purl.obolibrary.org/obo/GAZ_00236950 -->

    <owl:NamedIndividual rdf:about="http://purl.obolibrary.org/obo/GAZ_00236950">
        <obo:IAO_0000115>A fourth-level administrative division of Uganda.</obo:IAO_0000115>
        <oboInOwl:hasOBONamespace>GAZ</oboInOwl:hasOBONamespace>
        <oboInOwl:id>GAZ:00236950</oboInOwl:id>
        <rdfs:label>Kuluba Sub-county</rdfs:label>
    </owl:NamedIndividual>
    


    <!-- http://purl.obolibrary.org/obo/GAZ_00236951 -->

    <owl:NamedIndividual rdf:about="http://purl.obolibrary.org/obo/GAZ_00236951">
        <obo:IAO_0000115>A fourth-level administrative division of Uganda.</obo:IAO_0000115>
        <oboInOwl:hasOBONamespace>GAZ</oboInOwl:hasOBONamespace>
        <oboInOwl:id>GAZ:00236951</oboInOwl:id>
        <rdfs:label>Lobule Sub-county</rdfs:label>
    </owl:NamedIndividual>
    


    <!-- http://purl.obolibrary.org/obo/GAZ_00236952 -->

    <owl:NamedIndividual rdf:about="http://purl.obolibrary.org/obo/GAZ_00236952">
        <obo:IAO_0000115>A fourth-level administrative division of Uganda.</obo:IAO_0000115>
        <oboInOwl:hasOBONamespace>GAZ</oboInOwl:hasOBONamespace>
        <oboInOwl:id>GAZ:00236952</oboInOwl:id>
        <rdfs:label>Ludara Sub-county</rdfs:label>
    </owl:NamedIndividual>
    


    <!-- http://purl.obolibrary.org/obo/GAZ_00236953 -->

    <owl:NamedIndividual rdf:about="http://purl.obolibrary.org/obo/GAZ_00236953">
        <obo:IAO_0000115>A fourth-level administrative division of Uganda.</obo:IAO_0000115>
        <oboInOwl:hasOBONamespace>GAZ</oboInOwl:hasOBONamespace>
        <oboInOwl:id>GAZ:00236953</oboInOwl:id>
        <rdfs:label>Midia Sub-county</rdfs:label>
    </owl:NamedIndividual>
    


    <!-- http://purl.obolibrary.org/obo/GAZ_00236954 -->

    <owl:NamedIndividual rdf:about="http://purl.obolibrary.org/obo/GAZ_00236954">
        <obo:RO_0001025 rdf:resource="http://purl.obolibrary.org/obo/GAZ_00015492"/>
        <obo:IAO_0000115>A fourth-level administrative division of Uganda.</obo:IAO_0000115>
        <oboInOwl:hasOBONamespace>GAZ</oboInOwl:hasOBONamespace>
        <oboInOwl:id>GAZ:00236954</oboInOwl:id>
        <rdfs:label>Offaka Sub-county</rdfs:label>
    </owl:NamedIndividual>
    


    <!-- http://purl.obolibrary.org/obo/GAZ_00236955 -->

    <owl:NamedIndividual rdf:about="http://purl.obolibrary.org/obo/GAZ_00236955">
        <obo:RO_0001025 rdf:resource="http://purl.obolibrary.org/obo/GAZ_00015492"/>
        <obo:IAO_0000115>A fourth-level administrative division of Uganda.</obo:IAO_0000115>
        <oboInOwl:hasOBONamespace>GAZ</oboInOwl:hasOBONamespace>
        <oboInOwl:id>GAZ:00236955</oboInOwl:id>
        <rdfs:label>Ogoko Sub-county</rdfs:label>
    </owl:NamedIndividual>
    


    <!-- http://purl.obolibrary.org/obo/GAZ_00236956 -->

    <owl:NamedIndividual rdf:about="http://purl.obolibrary.org/obo/GAZ_00236956">
        <obo:RO_0001025 rdf:resource="http://purl.obolibrary.org/obo/GAZ_00015492"/>
        <obo:IAO_0000115>A fourth-level administrative division of Uganda.</obo:IAO_0000115>
        <oboInOwl:hasOBONamespace>GAZ</oboInOwl:hasOBONamespace>
        <oboInOwl:id>GAZ:00236956</oboInOwl:id>
        <rdfs:label>Okollo Sub-county</rdfs:label>
    </owl:NamedIndividual>
    


    <!-- http://purl.obolibrary.org/obo/GAZ_00236957 -->

    <owl:NamedIndividual rdf:about="http://purl.obolibrary.org/obo/GAZ_00236957">
        <obo:RO_0001025 rdf:resource="http://purl.obolibrary.org/obo/GAZ_00015492"/>
        <obo:IAO_0000115>A fourth-level administrative division of Uganda.</obo:IAO_0000115>
        <oboInOwl:hasOBONamespace>GAZ</oboInOwl:hasOBONamespace>
        <oboInOwl:id>GAZ:00236957</oboInOwl:id>
        <rdfs:label>Rhino Camp Sub-county</rdfs:label>
    </owl:NamedIndividual>
    


    <!-- http://purl.obolibrary.org/obo/GAZ_00236958 -->

    <owl:NamedIndividual rdf:about="http://purl.obolibrary.org/obo/GAZ_00236958">
        <obo:RO_0001025 rdf:resource="http://purl.obolibrary.org/obo/GAZ_00015492"/>
        <obo:IAO_0000115>A fourth-level administrative division of Uganda.</obo:IAO_0000115>
        <oboInOwl:hasOBONamespace>GAZ</oboInOwl:hasOBONamespace>
        <oboInOwl:id>GAZ:00236958</oboInOwl:id>
        <rdfs:label>Rigbo Sub-county</rdfs:label>
    </owl:NamedIndividual>
    


    <!-- http://purl.obolibrary.org/obo/GAZ_00236959 -->

    <owl:NamedIndividual rdf:about="http://purl.obolibrary.org/obo/GAZ_00236959">
        <obo:RO_0001025 rdf:resource="http://purl.obolibrary.org/obo/GAZ_00015492"/>
        <obo:IAO_0000115>A fourth-level administrative division of Uganda.</obo:IAO_0000115>
        <oboInOwl:hasOBONamespace>GAZ</oboInOwl:hasOBONamespace>
        <oboInOwl:id>GAZ:00236959</oboInOwl:id>
        <rdfs:label>Uleppi Sub-county</rdfs:label>
    </owl:NamedIndividual>
    


    <!-- http://purl.obolibrary.org/obo/GAZ_00236960 -->

    <owl:NamedIndividual rdf:about="http://purl.obolibrary.org/obo/GAZ_00236960">
        <obo:RO_0001025 rdf:resource="http://purl.obolibrary.org/obo/GAZ_00015508"/>
        <obo:IAO_0000115>A fourth-level administrative division of Uganda.</obo:IAO_0000115>
        <oboInOwl:hasOBONamespace>GAZ</oboInOwl:hasOBONamespace>
        <oboInOwl:id>GAZ:00236960</oboInOwl:id>
        <rdfs:label>Yivu Sub-county</rdfs:label>
    </owl:NamedIndividual>
    


    <!-- http://purl.obolibrary.org/obo/GAZ_00236961 -->

    <owl:NamedIndividual rdf:about="http://purl.obolibrary.org/obo/GAZ_00236961">
        <obo:RO_0001025 rdf:resource="http://purl.obolibrary.org/obo/GAZ_00015508"/>
        <obo:IAO_0000115>A fourth-level administrative division of Uganda.</obo:IAO_0000115>
        <oboInOwl:hasOBONamespace>GAZ</oboInOwl:hasOBONamespace>
        <oboInOwl:id>GAZ:00236961</oboInOwl:id>
        <rdfs:label>Nyadri Sub-county</rdfs:label>
    </owl:NamedIndividual>
    


    <!-- http://purl.obolibrary.org/obo/GAZ_00236962 -->

    <owl:NamedIndividual rdf:about="http://purl.obolibrary.org/obo/GAZ_00236962">
        <obo:RO_0001025 rdf:resource="http://purl.obolibrary.org/obo/GAZ_00015508"/>
        <obo:IAO_0000115>A fourth-level administrative division of Uganda.</obo:IAO_0000115>
        <oboInOwl:hasOBONamespace>GAZ</oboInOwl:hasOBONamespace>
        <oboInOwl:id>GAZ:00236962</oboInOwl:id>
        <rdfs:label>Oleba Sub-county</rdfs:label>
    </owl:NamedIndividual>
    


    <!-- http://purl.obolibrary.org/obo/GAZ_00236963 -->

    <owl:NamedIndividual rdf:about="http://purl.obolibrary.org/obo/GAZ_00236963">
        <obo:RO_0001025 rdf:resource="http://purl.obolibrary.org/obo/GAZ_00015508"/>
        <obo:IAO_0000115>A fourth-level administrative division of Uganda.</obo:IAO_0000115>
        <oboInOwl:hasOBONamespace>GAZ</oboInOwl:hasOBONamespace>
        <oboInOwl:id>GAZ:00236963</oboInOwl:id>
        <rdfs:label>Oluvu Sub-county</rdfs:label>
    </owl:NamedIndividual>
    


    <!-- http://purl.obolibrary.org/obo/GAZ_00236964 -->

    <owl:NamedIndividual rdf:about="http://purl.obolibrary.org/obo/GAZ_00236964">
        <obo:RO_0001025 rdf:resource="http://purl.obolibrary.org/obo/GAZ_00015508"/>
        <obo:IAO_0000115>A fourth-level administrative division of Uganda.</obo:IAO_0000115>
        <oboInOwl:hasOBONamespace>GAZ</oboInOwl:hasOBONamespace>
        <oboInOwl:id>GAZ:00236964</oboInOwl:id>
        <rdfs:label>Tara Sub-county</rdfs:label>
    </owl:NamedIndividual>
    


    <!-- http://purl.obolibrary.org/obo/GAZ_00236965 -->

    <owl:NamedIndividual rdf:about="http://purl.obolibrary.org/obo/GAZ_00236965">
        <obo:RO_0001025 rdf:resource="http://purl.obolibrary.org/obo/GAZ_00015508"/>
        <obo:IAO_0000115>A fourth-level administrative division of Uganda.</obo:IAO_0000115>
        <oboInOwl:hasOBONamespace>GAZ</oboInOwl:hasOBONamespace>
        <oboInOwl:id>GAZ:00236965</oboInOwl:id>
        <rdfs:label>Oluffe Sub-county</rdfs:label>
    </owl:NamedIndividual>
    


    <!-- http://purl.obolibrary.org/obo/GAZ_00236966 -->

    <owl:NamedIndividual rdf:about="http://purl.obolibrary.org/obo/GAZ_00236966">
        <obo:RO_0001025 rdf:resource="http://purl.obolibrary.org/obo/GAZ_00015508"/>
        <obo:IAO_0000115>A fourth-level administrative division of Uganda.</obo:IAO_0000115>
        <oboInOwl:hasOBONamespace>GAZ</oboInOwl:hasOBONamespace>
        <oboInOwl:id>GAZ:00236966</oboInOwl:id>
        <rdfs:label>Kijomoro Sub-county</rdfs:label>
    </owl:NamedIndividual>
    


    <!-- http://purl.obolibrary.org/obo/GAZ_00236967 -->

    <owl:NamedIndividual rdf:about="http://purl.obolibrary.org/obo/GAZ_00236967">
        <obo:RO_0001025 rdf:resource="http://purl.obolibrary.org/obo/GAZ_00015508"/>
        <obo:IAO_0000115>A fourth-level administrative division of Uganda.</obo:IAO_0000115>
        <oboInOwl:hasOBONamespace>GAZ</oboInOwl:hasOBONamespace>
        <oboInOwl:id>GAZ:00236967</oboInOwl:id>
        <rdfs:label>Terego Sub-county</rdfs:label>
    </owl:NamedIndividual>
    


    <!-- http://purl.obolibrary.org/obo/GAZ_00236968 -->

    <owl:NamedIndividual rdf:about="http://purl.obolibrary.org/obo/GAZ_00236968">
        <obo:RO_0001025 rdf:resource="http://purl.obolibrary.org/obo/GAZ_00015508"/>
        <obo:IAO_0000115>A fourth-level administrative division of Uganda.</obo:IAO_0000115>
        <oboInOwl:hasOBONamespace>GAZ</oboInOwl:hasOBONamespace>
        <oboInOwl:id>GAZ:00236968</oboInOwl:id>
        <rdfs:label>Aii -Vu Sub-county</rdfs:label>
    </owl:NamedIndividual>
    


    <!-- http://purl.obolibrary.org/obo/GAZ_00236969 -->

    <owl:NamedIndividual rdf:about="http://purl.obolibrary.org/obo/GAZ_00236969">
        <obo:RO_0001025 rdf:resource="http://purl.obolibrary.org/obo/GAZ_00015508"/>
        <obo:IAO_0000115>A fourth-level administrative division of Uganda.</obo:IAO_0000115>
        <oboInOwl:hasOBONamespace>GAZ</oboInOwl:hasOBONamespace>
        <oboInOwl:id>GAZ:00236969</oboInOwl:id>
        <rdfs:label>Beleafe Sub-county</rdfs:label>
    </owl:NamedIndividual>
    


    <!-- http://purl.obolibrary.org/obo/GAZ_00236970 -->

    <owl:NamedIndividual rdf:about="http://purl.obolibrary.org/obo/GAZ_00236970">
        <obo:RO_0001025 rdf:resource="http://purl.obolibrary.org/obo/GAZ_00015508"/>
        <obo:IAO_0000115>A fourth-level administrative division of Uganda.</obo:IAO_0000115>
        <oboInOwl:hasOBONamespace>GAZ</oboInOwl:hasOBONamespace>
        <oboInOwl:id>GAZ:00236970</oboInOwl:id>
        <rdfs:label>Katrini Sub-county</rdfs:label>
    </owl:NamedIndividual>
    


    <!-- http://purl.obolibrary.org/obo/GAZ_00236971 -->

    <owl:NamedIndividual rdf:about="http://purl.obolibrary.org/obo/GAZ_00236971">
        <obo:RO_0001025 rdf:resource="http://purl.obolibrary.org/obo/GAZ_00015508"/>
        <obo:IAO_0000115>A fourth-level administrative division of Uganda.</obo:IAO_0000115>
        <oboInOwl:hasOBONamespace>GAZ</oboInOwl:hasOBONamespace>
        <oboInOwl:id>GAZ:00236971</oboInOwl:id>
        <rdfs:label>Odupi Sub-county</rdfs:label>
    </owl:NamedIndividual>
    


    <!-- http://purl.obolibrary.org/obo/GAZ_00236972 -->

    <owl:NamedIndividual rdf:about="http://purl.obolibrary.org/obo/GAZ_00236972">
        <obo:RO_0001025 rdf:resource="http://purl.obolibrary.org/obo/GAZ_00015508"/>
        <obo:IAO_0000115>A fourth-level administrative division of Uganda.</obo:IAO_0000115>
        <oboInOwl:hasOBONamespace>GAZ</oboInOwl:hasOBONamespace>
        <oboInOwl:id>GAZ:00236972</oboInOwl:id>
        <rdfs:label>Omugo Sub-county</rdfs:label>
    </owl:NamedIndividual>
    


    <!-- http://purl.obolibrary.org/obo/GAZ_00236973 -->

    <owl:NamedIndividual rdf:about="http://purl.obolibrary.org/obo/GAZ_00236973">
        <obo:RO_0001025 rdf:resource="http://purl.obolibrary.org/obo/GAZ_00015508"/>
        <obo:IAO_0000115>A fourth-level administrative division of Uganda.</obo:IAO_0000115>
        <oboInOwl:hasOBONamespace>GAZ</oboInOwl:hasOBONamespace>
        <oboInOwl:id>GAZ:00236973</oboInOwl:id>
        <rdfs:label>Uriama Sub-county</rdfs:label>
    </owl:NamedIndividual>
    


    <!-- http://purl.obolibrary.org/obo/GAZ_00236974 -->

    <owl:NamedIndividual rdf:about="http://purl.obolibrary.org/obo/GAZ_00236974">
        <obo:RO_0001025 rdf:resource="http://purl.obolibrary.org/obo/GAZ_00015494"/>
        <obo:IAO_0000115>A fourth-level administrative division of Uganda.</obo:IAO_0000115>
        <oboInOwl:hasOBONamespace>GAZ</oboInOwl:hasOBONamespace>
        <oboInOwl:id>GAZ:00236974</oboInOwl:id>
        <rdfs:label>Ajia Sub-county</rdfs:label>
    </owl:NamedIndividual>
    


    <!-- http://purl.obolibrary.org/obo/GAZ_00236975 -->

    <owl:NamedIndividual rdf:about="http://purl.obolibrary.org/obo/GAZ_00236975">
        <obo:RO_0001025 rdf:resource="http://purl.obolibrary.org/obo/GAZ_00015494"/>
        <obo:IAO_0000115>A fourth-level administrative division of Uganda.</obo:IAO_0000115>
        <oboInOwl:hasOBONamespace>GAZ</oboInOwl:hasOBONamespace>
        <oboInOwl:id>GAZ:00236975</oboInOwl:id>
        <rdfs:label>Arivu Sub-county</rdfs:label>
    </owl:NamedIndividual>
    


    <!-- http://purl.obolibrary.org/obo/GAZ_00236976 -->

    <owl:NamedIndividual rdf:about="http://purl.obolibrary.org/obo/GAZ_00236976">
        <obo:RO_0001025 rdf:resource="http://purl.obolibrary.org/obo/GAZ_00015494"/>
        <obo:IAO_0000115>A fourth-level administrative division of Uganda.</obo:IAO_0000115>
        <oboInOwl:hasOBONamespace>GAZ</oboInOwl:hasOBONamespace>
        <oboInOwl:id>GAZ:00236976</oboInOwl:id>
        <rdfs:label>Logiri Sub-county</rdfs:label>
    </owl:NamedIndividual>
    


    <!-- http://purl.obolibrary.org/obo/GAZ_00236977 -->

    <owl:NamedIndividual rdf:about="http://purl.obolibrary.org/obo/GAZ_00236977">
        <obo:RO_0001025 rdf:resource="http://purl.obolibrary.org/obo/GAZ_00015494"/>
        <obo:IAO_0000115>A fourth-level administrative division of Uganda.</obo:IAO_0000115>
        <oboInOwl:hasOBONamespace>GAZ</oboInOwl:hasOBONamespace>
        <oboInOwl:id>GAZ:00236977</oboInOwl:id>
        <rdfs:label>Vurra Sub-county</rdfs:label>
    </owl:NamedIndividual>
    


    <!-- http://purl.obolibrary.org/obo/GAZ_00236978 -->

    <owl:NamedIndividual rdf:about="http://purl.obolibrary.org/obo/GAZ_00236978">
        <obo:IAO_0000115>A fourth-level administrative division of Uganda.</obo:IAO_0000115>
        <oboInOwl:hasOBONamespace>GAZ</oboInOwl:hasOBONamespace>
        <oboInOwl:id>GAZ:00236978</oboInOwl:id>
        <rdfs:label>Agwata Sub-county</rdfs:label>
    </owl:NamedIndividual>
    


    <!-- http://purl.obolibrary.org/obo/GAZ_00236979 -->

    <owl:NamedIndividual rdf:about="http://purl.obolibrary.org/obo/GAZ_00236979">
        <obo:IAO_0000115>A fourth-level administrative division of Uganda.</obo:IAO_0000115>
        <oboInOwl:hasOBONamespace>GAZ</oboInOwl:hasOBONamespace>
        <oboInOwl:id>GAZ:00236979</oboInOwl:id>
        <rdfs:label>Batta Sub-county</rdfs:label>
    </owl:NamedIndividual>
    


    <!-- http://purl.obolibrary.org/obo/GAZ_00236980 -->

    <owl:NamedIndividual rdf:about="http://purl.obolibrary.org/obo/GAZ_00236980">
        <obo:IAO_0000115>A fourth-level administrative division of Uganda.</obo:IAO_0000115>
        <oboInOwl:hasOBONamespace>GAZ</oboInOwl:hasOBONamespace>
        <oboInOwl:id>GAZ:00236980</oboInOwl:id>
        <rdfs:label>Dokolo Sub-county</rdfs:label>
    </owl:NamedIndividual>
    


    <!-- http://purl.obolibrary.org/obo/GAZ_00236981 -->

    <owl:NamedIndividual rdf:about="http://purl.obolibrary.org/obo/GAZ_00236981">
        <obo:IAO_0000115>A fourth-level administrative division of Uganda.</obo:IAO_0000115>
        <oboInOwl:hasOBONamespace>GAZ</oboInOwl:hasOBONamespace>
        <oboInOwl:id>GAZ:00236981</oboInOwl:id>
        <rdfs:label>Kangai Sub-county</rdfs:label>
    </owl:NamedIndividual>
    


    <!-- http://purl.obolibrary.org/obo/GAZ_00236982 -->

    <owl:NamedIndividual rdf:about="http://purl.obolibrary.org/obo/GAZ_00236982">
        <obo:IAO_0000115>A fourth-level administrative division of Uganda.</obo:IAO_0000115>
        <oboInOwl:hasOBONamespace>GAZ</oboInOwl:hasOBONamespace>
        <oboInOwl:id>GAZ:00236982</oboInOwl:id>
        <rdfs:label>Kwera Sub-county</rdfs:label>
    </owl:NamedIndividual>
    


    <!-- http://purl.obolibrary.org/obo/GAZ_00236983 -->

    <owl:NamedIndividual rdf:about="http://purl.obolibrary.org/obo/GAZ_00236983">
        <obo:RO_0001025 rdf:resource="http://purl.obolibrary.org/obo/GAZ_00015507"/>
        <obo:IAO_0000115>A fourth-level administrative division of Uganda.</obo:IAO_0000115>
        <oboInOwl:hasOBONamespace>GAZ</oboInOwl:hasOBONamespace>
        <oboInOwl:id>GAZ:00236983</oboInOwl:id>
        <rdfs:label>Adekokwok Sub-county</rdfs:label>
    </owl:NamedIndividual>
    


    <!-- http://purl.obolibrary.org/obo/GAZ_00236984 -->

    <owl:NamedIndividual rdf:about="http://purl.obolibrary.org/obo/GAZ_00236984">
        <obo:RO_0001025 rdf:resource="http://purl.obolibrary.org/obo/GAZ_00015507"/>
        <obo:IAO_0000115>A fourth-level administrative division of Uganda.</obo:IAO_0000115>
        <oboInOwl:hasOBONamespace>GAZ</oboInOwl:hasOBONamespace>
        <oboInOwl:id>GAZ:00236984</oboInOwl:id>
        <rdfs:label>Amach Sub-county</rdfs:label>
    </owl:NamedIndividual>
    


    <!-- http://purl.obolibrary.org/obo/GAZ_00236985 -->

    <owl:NamedIndividual rdf:about="http://purl.obolibrary.org/obo/GAZ_00236985">
        <obo:RO_0001025 rdf:resource="http://purl.obolibrary.org/obo/GAZ_00015507"/>
        <obo:IAO_0000115>A fourth-level administrative division of Uganda.</obo:IAO_0000115>
        <oboInOwl:hasOBONamespace>GAZ</oboInOwl:hasOBONamespace>
        <oboInOwl:id>GAZ:00236985</oboInOwl:id>
        <rdfs:label>Aromo Sub-county</rdfs:label>
    </owl:NamedIndividual>
    


    <!-- http://purl.obolibrary.org/obo/GAZ_00236986 -->

    <owl:NamedIndividual rdf:about="http://purl.obolibrary.org/obo/GAZ_00236986">
        <obo:RO_0001025 rdf:resource="http://purl.obolibrary.org/obo/GAZ_00015507"/>
        <obo:IAO_0000115>A fourth-level administrative division of Uganda.</obo:IAO_0000115>
        <oboInOwl:hasOBONamespace>GAZ</oboInOwl:hasOBONamespace>
        <oboInOwl:id>GAZ:00236986</oboInOwl:id>
        <rdfs:label>Barr Sub-county</rdfs:label>
    </owl:NamedIndividual>
    


    <!-- http://purl.obolibrary.org/obo/GAZ_00236987 -->

    <owl:NamedIndividual rdf:about="http://purl.obolibrary.org/obo/GAZ_00236987">
        <obo:RO_0001025 rdf:resource="http://purl.obolibrary.org/obo/GAZ_00015507"/>
        <obo:IAO_0000115>A fourth-level administrative division of Uganda.</obo:IAO_0000115>
        <oboInOwl:hasOBONamespace>GAZ</oboInOwl:hasOBONamespace>
        <oboInOwl:id>GAZ:00236987</oboInOwl:id>
        <rdfs:label>Lira Sub-county</rdfs:label>
    </owl:NamedIndividual>
    


    <!-- http://purl.obolibrary.org/obo/GAZ_00236988 -->

    <owl:NamedIndividual rdf:about="http://purl.obolibrary.org/obo/GAZ_00236988">
        <obo:RO_0001025 rdf:resource="http://purl.obolibrary.org/obo/GAZ_00015507"/>
        <obo:IAO_0000115>A fourth-level administrative division of Uganda.</obo:IAO_0000115>
        <oboInOwl:hasOBONamespace>GAZ</oboInOwl:hasOBONamespace>
        <oboInOwl:id>GAZ:00236988</oboInOwl:id>
        <rdfs:label>Ogur Sub-county</rdfs:label>
    </owl:NamedIndividual>
    


    <!-- http://purl.obolibrary.org/obo/GAZ_00236989 -->

    <owl:NamedIndividual rdf:about="http://purl.obolibrary.org/obo/GAZ_00236989">
        <obo:RO_0001025 rdf:resource="http://purl.obolibrary.org/obo/GAZ_00015505"/>
        <obo:IAO_0000115>A fourth-level administrative division of Uganda.</obo:IAO_0000115>
        <oboInOwl:hasOBONamespace>GAZ</oboInOwl:hasOBONamespace>
        <oboInOwl:id>GAZ:00236989</oboInOwl:id>
        <rdfs:label>Adye Sub-county</rdfs:label>
    </owl:NamedIndividual>
    


    <!-- http://purl.obolibrary.org/obo/GAZ_00236990 -->

    <owl:NamedIndividual rdf:about="http://purl.obolibrary.org/obo/GAZ_00236990">
        <obo:RO_0001025 rdf:resource="http://purl.obolibrary.org/obo/GAZ_00015505"/>
        <obo:IAO_0000115>A fourth-level administrative division of Uganda.</obo:IAO_0000115>
        <oboInOwl:hasOBONamespace>GAZ</oboInOwl:hasOBONamespace>
        <oboInOwl:id>GAZ:00236990</oboInOwl:id>
        <rdfs:label>Central Sub-county</rdfs:label>
    </owl:NamedIndividual>
    


    <!-- http://purl.obolibrary.org/obo/GAZ_00236991 -->

    <owl:NamedIndividual rdf:about="http://purl.obolibrary.org/obo/GAZ_00236991">
        <obo:RO_0001025 rdf:resource="http://purl.obolibrary.org/obo/GAZ_00015505"/>
        <obo:IAO_0000115>A fourth-level administrative division of Uganda.</obo:IAO_0000115>
        <oboInOwl:hasOBONamespace>GAZ</oboInOwl:hasOBONamespace>
        <oboInOwl:id>GAZ:00236991</oboInOwl:id>
        <rdfs:label>Ojwina Sub-county</rdfs:label>
    </owl:NamedIndividual>
    


    <!-- http://purl.obolibrary.org/obo/GAZ_00236992 -->

    <owl:NamedIndividual rdf:about="http://purl.obolibrary.org/obo/GAZ_00236992">
        <obo:RO_0001025 rdf:resource="http://purl.obolibrary.org/obo/GAZ_00015505"/>
        <obo:IAO_0000115>A fourth-level administrative division of Uganda.</obo:IAO_0000115>
        <oboInOwl:hasOBONamespace>GAZ</oboInOwl:hasOBONamespace>
        <oboInOwl:id>GAZ:00236992</oboInOwl:id>
        <rdfs:label>Railway Sub-county</rdfs:label>
    </owl:NamedIndividual>
    


    <!-- http://purl.obolibrary.org/obo/GAZ_00236993 -->

    <owl:NamedIndividual rdf:about="http://purl.obolibrary.org/obo/GAZ_00236993">
        <obo:RO_0001025 rdf:resource="http://purl.obolibrary.org/obo/GAZ_00015506"/>
        <obo:IAO_0000115>A fourth-level administrative division of Uganda.</obo:IAO_0000115>
        <oboInOwl:hasOBONamespace>GAZ</oboInOwl:hasOBONamespace>
        <oboInOwl:id>GAZ:00236993</oboInOwl:id>
        <rdfs:label>Adwari Sub-county</rdfs:label>
    </owl:NamedIndividual>
    


    <!-- http://purl.obolibrary.org/obo/GAZ_00236994 -->

    <owl:NamedIndividual rdf:about="http://purl.obolibrary.org/obo/GAZ_00236994">
        <obo:RO_0001025 rdf:resource="http://purl.obolibrary.org/obo/GAZ_00015506"/>
        <obo:IAO_0000115>A fourth-level administrative division of Uganda.</obo:IAO_0000115>
        <oboInOwl:hasOBONamespace>GAZ</oboInOwl:hasOBONamespace>
        <oboInOwl:id>GAZ:00236994</oboInOwl:id>
        <rdfs:label>Okwang Sub-county</rdfs:label>
    </owl:NamedIndividual>
    


    <!-- http://purl.obolibrary.org/obo/GAZ_00236995 -->

    <owl:NamedIndividual rdf:about="http://purl.obolibrary.org/obo/GAZ_00236995">
        <obo:RO_0001025 rdf:resource="http://purl.obolibrary.org/obo/GAZ_00015506"/>
        <obo:IAO_0000115>A fourth-level administrative division of Uganda.</obo:IAO_0000115>
        <oboInOwl:hasOBONamespace>GAZ</oboInOwl:hasOBONamespace>
        <oboInOwl:id>GAZ:00236995</oboInOwl:id>
        <rdfs:label>Olilim Sub-county</rdfs:label>
    </owl:NamedIndividual>
    


    <!-- http://purl.obolibrary.org/obo/GAZ_00236996 -->

    <owl:NamedIndividual rdf:about="http://purl.obolibrary.org/obo/GAZ_00236996">
        <obo:RO_0001025 rdf:resource="http://purl.obolibrary.org/obo/GAZ_00015506"/>
        <obo:IAO_0000115>A fourth-level administrative division of Uganda.</obo:IAO_0000115>
        <oboInOwl:hasOBONamespace>GAZ</oboInOwl:hasOBONamespace>
        <oboInOwl:id>GAZ:00236996</oboInOwl:id>
        <rdfs:label>Orum Sub-county</rdfs:label>
    </owl:NamedIndividual>
    


    <!-- http://purl.obolibrary.org/obo/GAZ_00236997 -->

    <owl:NamedIndividual rdf:about="http://purl.obolibrary.org/obo/GAZ_00236997">
        <obo:RO_0001025 rdf:resource="http://purl.obolibrary.org/obo/GAZ_00015497"/>
        <obo:IAO_0000115>A fourth-level administrative division of Uganda.</obo:IAO_0000115>
        <oboInOwl:hasOBONamespace>GAZ</oboInOwl:hasOBONamespace>
        <oboInOwl:id>GAZ:00236997</oboInOwl:id>
        <rdfs:label>Awach Sub-county</rdfs:label>
    </owl:NamedIndividual>
    


    <!-- http://purl.obolibrary.org/obo/GAZ_00236998 -->

    <owl:NamedIndividual rdf:about="http://purl.obolibrary.org/obo/GAZ_00236998">
        <obo:RO_0001025 rdf:resource="http://purl.obolibrary.org/obo/GAZ_00015497"/>
        <obo:IAO_0000115>A fourth-level administrative division of Uganda.</obo:IAO_0000115>
        <oboInOwl:hasOBONamespace>GAZ</oboInOwl:hasOBONamespace>
        <oboInOwl:id>GAZ:00236998</oboInOwl:id>
        <rdfs:label>Bungatira Sub-county</rdfs:label>
    </owl:NamedIndividual>
    


    <!-- http://purl.obolibrary.org/obo/GAZ_00236999 -->

    <owl:NamedIndividual rdf:about="http://purl.obolibrary.org/obo/GAZ_00236999">
        <obo:RO_0001025 rdf:resource="http://purl.obolibrary.org/obo/GAZ_00015497"/>
        <obo:IAO_0000115>A fourth-level administrative division of Uganda.</obo:IAO_0000115>
        <oboInOwl:hasOBONamespace>GAZ</oboInOwl:hasOBONamespace>
        <oboInOwl:id>GAZ:00236999</oboInOwl:id>
        <rdfs:label>Paicho Sub-county</rdfs:label>
    </owl:NamedIndividual>
    


    <!-- http://purl.obolibrary.org/obo/GAZ_00237000 -->

    <owl:NamedIndividual rdf:about="http://purl.obolibrary.org/obo/GAZ_00237000">
        <obo:RO_0001025 rdf:resource="http://purl.obolibrary.org/obo/GAZ_00015497"/>
        <obo:IAO_0000115>A fourth-level administrative division of Uganda.</obo:IAO_0000115>
        <oboInOwl:hasOBONamespace>GAZ</oboInOwl:hasOBONamespace>
        <oboInOwl:id>GAZ:00237000</oboInOwl:id>
        <rdfs:label>Palaro Sub-county</rdfs:label>
    </owl:NamedIndividual>
    


    <!-- http://purl.obolibrary.org/obo/GAZ_00237001 -->

    <owl:NamedIndividual rdf:about="http://purl.obolibrary.org/obo/GAZ_00237001">
        <obo:RO_0001025 rdf:resource="http://purl.obolibrary.org/obo/GAZ_00015497"/>
        <obo:IAO_0000115>A fourth-level administrative division of Uganda.</obo:IAO_0000115>
        <oboInOwl:hasOBONamespace>GAZ</oboInOwl:hasOBONamespace>
        <oboInOwl:id>GAZ:00237001</oboInOwl:id>
        <rdfs:label>Patiko Sub-county</rdfs:label>
    </owl:NamedIndividual>
    


    <!-- http://purl.obolibrary.org/obo/GAZ_00237002 -->

    <owl:NamedIndividual rdf:about="http://purl.obolibrary.org/obo/GAZ_00237002">
        <obo:RO_0001025 rdf:resource="http://purl.obolibrary.org/obo/GAZ_00015498"/>
        <obo:IAO_0000115>A fourth-level administrative division of Uganda.</obo:IAO_0000115>
        <oboInOwl:hasOBONamespace>GAZ</oboInOwl:hasOBONamespace>
        <oboInOwl:id>GAZ:00237002</oboInOwl:id>
        <rdfs:label>Bobi Sub-county</rdfs:label>
    </owl:NamedIndividual>
    


    <!-- http://purl.obolibrary.org/obo/GAZ_00237003 -->

    <owl:NamedIndividual rdf:about="http://purl.obolibrary.org/obo/GAZ_00237003">
        <obo:RO_0001025 rdf:resource="http://purl.obolibrary.org/obo/GAZ_00015498"/>
        <obo:IAO_0000115>A fourth-level administrative division of Uganda.</obo:IAO_0000115>
        <oboInOwl:hasOBONamespace>GAZ</oboInOwl:hasOBONamespace>
        <oboInOwl:id>GAZ:00237003</oboInOwl:id>
        <rdfs:label>Koro Sub-county</rdfs:label>
    </owl:NamedIndividual>
    


    <!-- http://purl.obolibrary.org/obo/GAZ_00237004 -->

    <owl:NamedIndividual rdf:about="http://purl.obolibrary.org/obo/GAZ_00237004">
        <obo:RO_0001025 rdf:resource="http://purl.obolibrary.org/obo/GAZ_00015498"/>
        <obo:IAO_0000115>A fourth-level administrative division of Uganda.</obo:IAO_0000115>
        <oboInOwl:hasOBONamespace>GAZ</oboInOwl:hasOBONamespace>
        <oboInOwl:id>GAZ:00237004</oboInOwl:id>
        <rdfs:label>Lakwana Sub-county</rdfs:label>
    </owl:NamedIndividual>
    


    <!-- http://purl.obolibrary.org/obo/GAZ_00237005 -->

    <owl:NamedIndividual rdf:about="http://purl.obolibrary.org/obo/GAZ_00237005">
        <obo:RO_0001025 rdf:resource="http://purl.obolibrary.org/obo/GAZ_00015498"/>
        <obo:IAO_0000115>A fourth-level administrative division of Uganda.</obo:IAO_0000115>
        <oboInOwl:hasOBONamespace>GAZ</oboInOwl:hasOBONamespace>
        <oboInOwl:id>GAZ:00237005</oboInOwl:id>
        <rdfs:label>Lalogi Sub-county</rdfs:label>
    </owl:NamedIndividual>
    


    <!-- http://purl.obolibrary.org/obo/GAZ_00237006 -->

    <owl:NamedIndividual rdf:about="http://purl.obolibrary.org/obo/GAZ_00237006">
        <obo:RO_0001025 rdf:resource="http://purl.obolibrary.org/obo/GAZ_00015498"/>
        <obo:IAO_0000115>A fourth-level administrative division of Uganda.</obo:IAO_0000115>
        <oboInOwl:hasOBONamespace>GAZ</oboInOwl:hasOBONamespace>
        <oboInOwl:id>GAZ:00237006</oboInOwl:id>
        <rdfs:label>Odek Sub-county</rdfs:label>
    </owl:NamedIndividual>
    


    <!-- http://purl.obolibrary.org/obo/GAZ_00237007 -->

    <owl:NamedIndividual rdf:about="http://purl.obolibrary.org/obo/GAZ_00237007">
        <obo:RO_0001025 rdf:resource="http://purl.obolibrary.org/obo/GAZ_00015498"/>
        <obo:IAO_0000115>A fourth-level administrative division of Uganda.</obo:IAO_0000115>
        <oboInOwl:hasOBONamespace>GAZ</oboInOwl:hasOBONamespace>
        <oboInOwl:id>GAZ:00237007</oboInOwl:id>
        <rdfs:label>Ongako Sub-county</rdfs:label>
    </owl:NamedIndividual>
    


    <!-- http://purl.obolibrary.org/obo/GAZ_00237008 -->

    <owl:NamedIndividual rdf:about="http://purl.obolibrary.org/obo/GAZ_00237008">
        <obo:RO_0001025 rdf:resource="http://purl.obolibrary.org/obo/GAZ_00009914"/>
        <obo:IAO_0000115>A fourth-level administrative division of Uganda.</obo:IAO_0000115>
        <oboInOwl:hasOBONamespace>GAZ</oboInOwl:hasOBONamespace>
        <oboInOwl:id>GAZ:00237008</oboInOwl:id>
        <rdfs:label>Bar-dege Division</rdfs:label>
    </owl:NamedIndividual>
    


    <!-- http://purl.obolibrary.org/obo/GAZ_00237009 -->

    <owl:NamedIndividual rdf:about="http://purl.obolibrary.org/obo/GAZ_00237009">
        <obo:RO_0001025 rdf:resource="http://purl.obolibrary.org/obo/GAZ_00009914"/>
        <obo:IAO_0000115>A fourth-level administrative division of Uganda.</obo:IAO_0000115>
        <oboInOwl:hasOBONamespace>GAZ</oboInOwl:hasOBONamespace>
        <oboInOwl:id>GAZ:00237009</oboInOwl:id>
        <rdfs:label>Laroo Division</rdfs:label>
    </owl:NamedIndividual>
    


    <!-- http://purl.obolibrary.org/obo/GAZ_00237010 -->

    <owl:NamedIndividual rdf:about="http://purl.obolibrary.org/obo/GAZ_00237010">
        <obo:RO_0001025 rdf:resource="http://purl.obolibrary.org/obo/GAZ_00009914"/>
        <obo:IAO_0000115>A fourth-level administrative division of Uganda.</obo:IAO_0000115>
        <oboInOwl:hasOBONamespace>GAZ</oboInOwl:hasOBONamespace>
        <oboInOwl:id>GAZ:00237010</oboInOwl:id>
        <rdfs:label>Layibi Division</rdfs:label>
    </owl:NamedIndividual>
    


    <!-- http://purl.obolibrary.org/obo/GAZ_00237011 -->

    <owl:NamedIndividual rdf:about="http://purl.obolibrary.org/obo/GAZ_00237011">
        <obo:RO_0001025 rdf:resource="http://purl.obolibrary.org/obo/GAZ_00009914"/>
        <obo:IAO_0000115>A fourth-level administrative division of Uganda.</obo:IAO_0000115>
        <oboInOwl:hasOBONamespace>GAZ</oboInOwl:hasOBONamespace>
        <oboInOwl:id>GAZ:00237011</oboInOwl:id>
        <rdfs:label>Pece Division</rdfs:label>
    </owl:NamedIndividual>
    


    <!-- http://purl.obolibrary.org/obo/GAZ_00237013 -->

    <owl:NamedIndividual rdf:about="http://purl.obolibrary.org/obo/GAZ_00237013">
        <obo:IAO_0000115>A fourth-level administrative division of Uganda.</obo:IAO_0000115>
        <oboInOwl:hasOBONamespace>GAZ</oboInOwl:hasOBONamespace>
        <oboInOwl:id>GAZ:00237013</oboInOwl:id>
        <rdfs:label>Kaabong Town</rdfs:label>
    </owl:NamedIndividual>
    


    <!-- http://purl.obolibrary.org/obo/GAZ_00237014 -->

    <owl:NamedIndividual rdf:about="http://purl.obolibrary.org/obo/GAZ_00237014">
        <obo:IAO_0000115>A fourth-level administrative division of Uganda.</obo:IAO_0000115>
        <oboInOwl:hasOBONamespace>GAZ</oboInOwl:hasOBONamespace>
        <oboInOwl:id>GAZ:00237014</oboInOwl:id>
        <rdfs:label>Kalapata Sub-county</rdfs:label>
    </owl:NamedIndividual>
    


    <!-- http://purl.obolibrary.org/obo/GAZ_00237015 -->

    <owl:NamedIndividual rdf:about="http://purl.obolibrary.org/obo/GAZ_00237015">
        <obo:IAO_0000115>A fourth-level administrative division of Uganda.</obo:IAO_0000115>
        <oboInOwl:hasOBONamespace>GAZ</oboInOwl:hasOBONamespace>
        <oboInOwl:id>GAZ:00237015</oboInOwl:id>
        <rdfs:label>Kapedo Sub-county</rdfs:label>
    </owl:NamedIndividual>
    


    <!-- http://purl.obolibrary.org/obo/GAZ_00237016 -->

    <owl:NamedIndividual rdf:about="http://purl.obolibrary.org/obo/GAZ_00237016">
        <obo:IAO_0000115>A fourth-level administrative division of Uganda.</obo:IAO_0000115>
        <oboInOwl:hasOBONamespace>GAZ</oboInOwl:hasOBONamespace>
        <oboInOwl:id>GAZ:00237016</oboInOwl:id>
        <rdfs:label>Karenga Sub-county</rdfs:label>
    </owl:NamedIndividual>
    


    <!-- http://purl.obolibrary.org/obo/GAZ_00237017 -->

    <owl:NamedIndividual rdf:about="http://purl.obolibrary.org/obo/GAZ_00237017">
        <obo:IAO_0000115>A fourth-level administrative division of Uganda.</obo:IAO_0000115>
        <oboInOwl:hasOBONamespace>GAZ</oboInOwl:hasOBONamespace>
        <oboInOwl:id>GAZ:00237017</oboInOwl:id>
        <rdfs:label>Kathile Sub-county</rdfs:label>
    </owl:NamedIndividual>
    


    <!-- http://purl.obolibrary.org/obo/GAZ_00237018 -->

    <owl:NamedIndividual rdf:about="http://purl.obolibrary.org/obo/GAZ_00237018">
        <obo:IAO_0000115>A fourth-level administrative division of Uganda.</obo:IAO_0000115>
        <oboInOwl:hasOBONamespace>GAZ</oboInOwl:hasOBONamespace>
        <oboInOwl:id>GAZ:00237018</oboInOwl:id>
        <rdfs:label>Lolelia Sub-county</rdfs:label>
    </owl:NamedIndividual>
    


    <!-- http://purl.obolibrary.org/obo/GAZ_00237019 -->

    <owl:NamedIndividual rdf:about="http://purl.obolibrary.org/obo/GAZ_00237019">
        <obo:IAO_0000115>A fourth-level administrative division of Uganda.</obo:IAO_0000115>
        <oboInOwl:hasOBONamespace>GAZ</oboInOwl:hasOBONamespace>
        <oboInOwl:id>GAZ:00237019</oboInOwl:id>
        <rdfs:label>Loyoro Sub-county</rdfs:label>
    </owl:NamedIndividual>
    


    <!-- http://purl.obolibrary.org/obo/GAZ_00237020 -->

    <owl:NamedIndividual rdf:about="http://purl.obolibrary.org/obo/GAZ_00237020">
        <obo:IAO_0000115>A fourth-level administrative division of Uganda.</obo:IAO_0000115>
        <oboInOwl:hasOBONamespace>GAZ</oboInOwl:hasOBONamespace>
        <oboInOwl:id>GAZ:00237020</oboInOwl:id>
        <rdfs:label>Sidok Sub-county</rdfs:label>
    </owl:NamedIndividual>
    


    <!-- http://purl.obolibrary.org/obo/GAZ_00237021 -->

    <owl:NamedIndividual rdf:about="http://purl.obolibrary.org/obo/GAZ_00237021">
        <obo:IAO_0000115>A fourth-level administrative division of Uganda.</obo:IAO_0000115>
        <oboInOwl:hasOBONamespace>GAZ</oboInOwl:hasOBONamespace>
        <oboInOwl:id>GAZ:00237021</oboInOwl:id>
        <rdfs:label>Kaabong Sub-county</rdfs:label>
    </owl:NamedIndividual>
    


    <!-- http://purl.obolibrary.org/obo/GAZ_00237022 -->

    <owl:NamedIndividual rdf:about="http://purl.obolibrary.org/obo/GAZ_00237022">
        <obo:RO_0001025 rdf:resource="http://purl.obolibrary.org/obo/GAZ_00015503"/>
        <obo:IAO_0000115>A fourth-level administrative division of Uganda.</obo:IAO_0000115>
        <oboInOwl:hasOBONamespace>GAZ</oboInOwl:hasOBONamespace>
        <oboInOwl:id>GAZ:00237022</oboInOwl:id>
        <rdfs:label>Kacheri Sub-county</rdfs:label>
    </owl:NamedIndividual>
    


    <!-- http://purl.obolibrary.org/obo/GAZ_00237023 -->

    <owl:NamedIndividual rdf:about="http://purl.obolibrary.org/obo/GAZ_00237023">
        <obo:RO_0001025 rdf:resource="http://purl.obolibrary.org/obo/GAZ_00015503"/>
        <obo:IAO_0000115>A fourth-level administrative division of Uganda.</obo:IAO_0000115>
        <oboInOwl:hasOBONamespace>GAZ</oboInOwl:hasOBONamespace>
        <oboInOwl:id>GAZ:00237023</oboInOwl:id>
        <rdfs:label>Kotido Sub-county</rdfs:label>
    </owl:NamedIndividual>
    


    <!-- http://purl.obolibrary.org/obo/GAZ_00237024 -->

    <owl:NamedIndividual rdf:about="http://purl.obolibrary.org/obo/GAZ_00237024">
        <obo:RO_0001025 rdf:resource="http://purl.obolibrary.org/obo/GAZ_00015503"/>
        <obo:IAO_0000115>A fourth-level administrative division of Uganda.</obo:IAO_0000115>
        <oboInOwl:hasOBONamespace>GAZ</oboInOwl:hasOBONamespace>
        <oboInOwl:id>GAZ:00237024</oboInOwl:id>
        <rdfs:label>Kotido Town</rdfs:label>
    </owl:NamedIndividual>
    


    <!-- http://purl.obolibrary.org/obo/GAZ_00237025 -->

    <owl:NamedIndividual rdf:about="http://purl.obolibrary.org/obo/GAZ_00237025">
        <obo:RO_0001025 rdf:resource="http://purl.obolibrary.org/obo/GAZ_00015503"/>
        <obo:IAO_0000115>A fourth-level administrative division of Uganda.</obo:IAO_0000115>
        <oboInOwl:hasOBONamespace>GAZ</oboInOwl:hasOBONamespace>
        <oboInOwl:id>GAZ:00237025</oboInOwl:id>
        <rdfs:label>Nakapelimoru Sub-county</rdfs:label>
    </owl:NamedIndividual>
    


    <!-- http://purl.obolibrary.org/obo/GAZ_00237026 -->

    <owl:NamedIndividual rdf:about="http://purl.obolibrary.org/obo/GAZ_00237026">
        <obo:RO_0001025 rdf:resource="http://purl.obolibrary.org/obo/GAZ_00015503"/>
        <obo:IAO_0000115>A fourth-level administrative division of Uganda.</obo:IAO_0000115>
        <oboInOwl:hasOBONamespace>GAZ</oboInOwl:hasOBONamespace>
        <oboInOwl:id>GAZ:00237026</oboInOwl:id>
        <rdfs:label>Panyangara Sub-county</rdfs:label>
    </owl:NamedIndividual>
    


    <!-- http://purl.obolibrary.org/obo/GAZ_00237027 -->

    <owl:NamedIndividual rdf:about="http://purl.obolibrary.org/obo/GAZ_00237027">
        <obo:RO_0001025 rdf:resource="http://purl.obolibrary.org/obo/GAZ_00015503"/>
        <obo:IAO_0000115>A fourth-level administrative division of Uganda.</obo:IAO_0000115>
        <oboInOwl:hasOBONamespace>GAZ</oboInOwl:hasOBONamespace>
        <oboInOwl:id>GAZ:00237027</oboInOwl:id>
        <rdfs:label>Rengen Sub-county</rdfs:label>
    </owl:NamedIndividual>
    


    <!-- http://purl.obolibrary.org/obo/GAZ_00237028 -->

    <owl:NamedIndividual rdf:about="http://purl.obolibrary.org/obo/GAZ_00237028">
        <obo:RO_0001025 rdf:resource="http://purl.obolibrary.org/obo/GAZ_00015500"/>
        <obo:IAO_0000115>A fourth-level administrative division of Uganda.</obo:IAO_0000115>
        <oboInOwl:hasOBONamespace>GAZ</oboInOwl:hasOBONamespace>
        <oboInOwl:id>GAZ:00237028</oboInOwl:id>
        <rdfs:label>Kitgum Town</rdfs:label>
    </owl:NamedIndividual>
    


    <!-- http://purl.obolibrary.org/obo/GAZ_00237029 -->

    <owl:NamedIndividual rdf:about="http://purl.obolibrary.org/obo/GAZ_00237029">
        <obo:RO_0001025 rdf:resource="http://purl.obolibrary.org/obo/GAZ_00015500"/>
        <obo:IAO_0000115>A fourth-level administrative division of Uganda.</obo:IAO_0000115>
        <oboInOwl:hasOBONamespace>GAZ</oboInOwl:hasOBONamespace>
        <oboInOwl:id>GAZ:00237029</oboInOwl:id>
        <rdfs:label>Kitigum Matidi Sub-county</rdfs:label>
    </owl:NamedIndividual>
    


    <!-- http://purl.obolibrary.org/obo/GAZ_00237030 -->

    <owl:NamedIndividual rdf:about="http://purl.obolibrary.org/obo/GAZ_00237030">
        <obo:RO_0001025 rdf:resource="http://purl.obolibrary.org/obo/GAZ_00015500"/>
        <obo:IAO_0000115>A fourth-level administrative division of Uganda.</obo:IAO_0000115>
        <oboInOwl:hasOBONamespace>GAZ</oboInOwl:hasOBONamespace>
        <oboInOwl:id>GAZ:00237030</oboInOwl:id>
        <rdfs:label>Labongo Akwang Sub-county</rdfs:label>
    </owl:NamedIndividual>
    


    <!-- http://purl.obolibrary.org/obo/GAZ_00237031 -->

    <owl:NamedIndividual rdf:about="http://purl.obolibrary.org/obo/GAZ_00237031">
        <obo:RO_0001025 rdf:resource="http://purl.obolibrary.org/obo/GAZ_00015500"/>
        <obo:IAO_0000115>A fourth-level administrative division of Uganda.</obo:IAO_0000115>
        <oboInOwl:hasOBONamespace>GAZ</oboInOwl:hasOBONamespace>
        <oboInOwl:id>GAZ:00237031</oboInOwl:id>
        <rdfs:label>Labongo Amida Sub-county</rdfs:label>
    </owl:NamedIndividual>
    


    <!-- http://purl.obolibrary.org/obo/GAZ_00237032 -->

    <owl:NamedIndividual rdf:about="http://purl.obolibrary.org/obo/GAZ_00237032">
        <obo:RO_0001025 rdf:resource="http://purl.obolibrary.org/obo/GAZ_00015500"/>
        <obo:IAO_0000115>A fourth-level administrative division of Uganda.</obo:IAO_0000115>
        <oboInOwl:hasOBONamespace>GAZ</oboInOwl:hasOBONamespace>
        <oboInOwl:id>GAZ:00237032</oboInOwl:id>
        <rdfs:label>Labongo Layamo Sub-county</rdfs:label>
    </owl:NamedIndividual>
    


    <!-- http://purl.obolibrary.org/obo/GAZ_00237033 -->

    <owl:NamedIndividual rdf:about="http://purl.obolibrary.org/obo/GAZ_00237033">
        <obo:RO_0001025 rdf:resource="http://purl.obolibrary.org/obo/GAZ_00015500"/>
        <obo:IAO_0000115>A fourth-level administrative division of Uganda.</obo:IAO_0000115>
        <oboInOwl:hasOBONamespace>GAZ</oboInOwl:hasOBONamespace>
        <oboInOwl:id>GAZ:00237033</oboInOwl:id>
        <rdfs:label>Lagoro Sub-county</rdfs:label>
    </owl:NamedIndividual>
    


    <!-- http://purl.obolibrary.org/obo/GAZ_00237034 -->

    <owl:NamedIndividual rdf:about="http://purl.obolibrary.org/obo/GAZ_00237034">
        <obo:RO_0001025 rdf:resource="http://purl.obolibrary.org/obo/GAZ_00015500"/>
        <obo:IAO_0000115>A fourth-level administrative division of Uganda.</obo:IAO_0000115>
        <oboInOwl:hasOBONamespace>GAZ</oboInOwl:hasOBONamespace>
        <oboInOwl:id>GAZ:00237034</oboInOwl:id>
        <rdfs:label>Mucwini Sub-county</rdfs:label>
    </owl:NamedIndividual>
    


    <!-- http://purl.obolibrary.org/obo/GAZ_00237035 -->

    <owl:NamedIndividual rdf:about="http://purl.obolibrary.org/obo/GAZ_00237035">
        <obo:RO_0001025 rdf:resource="http://purl.obolibrary.org/obo/GAZ_00015500"/>
        <obo:IAO_0000115>A fourth-level administrative division of Uganda.</obo:IAO_0000115>
        <oboInOwl:hasOBONamespace>GAZ</oboInOwl:hasOBONamespace>
        <oboInOwl:id>GAZ:00237035</oboInOwl:id>
        <rdfs:label>Namokora Sub-county</rdfs:label>
    </owl:NamedIndividual>
    


    <!-- http://purl.obolibrary.org/obo/GAZ_00237036 -->

    <owl:NamedIndividual rdf:about="http://purl.obolibrary.org/obo/GAZ_00237036">
        <obo:RO_0001025 rdf:resource="http://purl.obolibrary.org/obo/GAZ_00015500"/>
        <obo:IAO_0000115>A fourth-level administrative division of Uganda.</obo:IAO_0000115>
        <oboInOwl:hasOBONamespace>GAZ</oboInOwl:hasOBONamespace>
        <oboInOwl:id>GAZ:00237036</oboInOwl:id>
        <rdfs:label>Omiya Anyima Sub-county</rdfs:label>
    </owl:NamedIndividual>
    


    <!-- http://purl.obolibrary.org/obo/GAZ_00237037 -->

    <owl:NamedIndividual rdf:about="http://purl.obolibrary.org/obo/GAZ_00237037">
        <obo:RO_0001025 rdf:resource="http://purl.obolibrary.org/obo/GAZ_00015500"/>
        <obo:IAO_0000115>A fourth-level administrative division of Uganda.</obo:IAO_0000115>
        <oboInOwl:hasOBONamespace>GAZ</oboInOwl:hasOBONamespace>
        <oboInOwl:id>GAZ:00237037</oboInOwl:id>
        <rdfs:label>Orom Sub-county</rdfs:label>
    </owl:NamedIndividual>
    


    <!-- http://purl.obolibrary.org/obo/GAZ_00237038 -->

    <owl:NamedIndividual rdf:about="http://purl.obolibrary.org/obo/GAZ_00237038">
        <obo:RO_0001025 rdf:resource="http://purl.obolibrary.org/obo/GAZ_00015501"/>
        <obo:IAO_0000115>A fourth-level administrative division of Uganda.</obo:IAO_0000115>
        <oboInOwl:hasOBONamespace>GAZ</oboInOwl:hasOBONamespace>
        <oboInOwl:id>GAZ:00237038</oboInOwl:id>
        <rdfs:label>Agoro Sub-county</rdfs:label>
    </owl:NamedIndividual>
    


    <!-- http://purl.obolibrary.org/obo/GAZ_00237039 -->

    <owl:NamedIndividual rdf:about="http://purl.obolibrary.org/obo/GAZ_00237039">
        <obo:RO_0001025 rdf:resource="http://purl.obolibrary.org/obo/GAZ_00015501"/>
        <obo:IAO_0000115>A fourth-level administrative division of Uganda.</obo:IAO_0000115>
        <oboInOwl:hasOBONamespace>GAZ</oboInOwl:hasOBONamespace>
        <oboInOwl:id>GAZ:00237039</oboInOwl:id>
        <rdfs:label>Lokung Sub-county</rdfs:label>
    </owl:NamedIndividual>
    


    <!-- http://purl.obolibrary.org/obo/GAZ_00237040 -->

    <owl:NamedIndividual rdf:about="http://purl.obolibrary.org/obo/GAZ_00237040">
        <obo:RO_0001025 rdf:resource="http://purl.obolibrary.org/obo/GAZ_00015501"/>
        <obo:IAO_0000115>A fourth-level administrative division of Uganda.</obo:IAO_0000115>
        <oboInOwl:hasOBONamespace>GAZ</oboInOwl:hasOBONamespace>
        <oboInOwl:id>GAZ:00237040</oboInOwl:id>
        <rdfs:label>Madi Opei Sub-county</rdfs:label>
    </owl:NamedIndividual>
    


    <!-- http://purl.obolibrary.org/obo/GAZ_00237041 -->

    <owl:NamedIndividual rdf:about="http://purl.obolibrary.org/obo/GAZ_00237041">
        <obo:RO_0001025 rdf:resource="http://purl.obolibrary.org/obo/GAZ_00015501"/>
        <obo:IAO_0000115>A fourth-level administrative division of Uganda.</obo:IAO_0000115>
        <oboInOwl:hasOBONamespace>GAZ</oboInOwl:hasOBONamespace>
        <oboInOwl:id>GAZ:00237041</oboInOwl:id>
        <rdfs:label>Parabek Ogili Sub-county</rdfs:label>
    </owl:NamedIndividual>
    


    <!-- http://purl.obolibrary.org/obo/GAZ_00237042 -->

    <owl:NamedIndividual rdf:about="http://purl.obolibrary.org/obo/GAZ_00237042">
        <obo:RO_0001025 rdf:resource="http://purl.obolibrary.org/obo/GAZ_00015501"/>
        <obo:IAO_0000115>A fourth-level administrative division of Uganda.</obo:IAO_0000115>
        <oboInOwl:hasOBONamespace>GAZ</oboInOwl:hasOBONamespace>
        <oboInOwl:id>GAZ:00237042</oboInOwl:id>
        <rdfs:label>Padibe East Sub-county</rdfs:label>
    </owl:NamedIndividual>
    


    <!-- http://purl.obolibrary.org/obo/GAZ_00237043 -->

    <owl:NamedIndividual rdf:about="http://purl.obolibrary.org/obo/GAZ_00237043">
        <obo:RO_0001025 rdf:resource="http://purl.obolibrary.org/obo/GAZ_00015501"/>
        <obo:IAO_0000115>A fourth-level administrative division of Uganda.</obo:IAO_0000115>
        <oboInOwl:hasOBONamespace>GAZ</oboInOwl:hasOBONamespace>
        <oboInOwl:id>GAZ:00237043</oboInOwl:id>
        <rdfs:label>Padibe West Sub-county</rdfs:label>
    </owl:NamedIndividual>
    


    <!-- http://purl.obolibrary.org/obo/GAZ_00237044 -->

    <owl:NamedIndividual rdf:about="http://purl.obolibrary.org/obo/GAZ_00237044">
        <obo:RO_0001025 rdf:resource="http://purl.obolibrary.org/obo/GAZ_00015501"/>
        <obo:IAO_0000115>A fourth-level administrative division of Uganda.</obo:IAO_0000115>
        <oboInOwl:hasOBONamespace>GAZ</oboInOwl:hasOBONamespace>
        <oboInOwl:id>GAZ:00237044</oboInOwl:id>
        <rdfs:label>Palabek Gem Sub-county</rdfs:label>
    </owl:NamedIndividual>
    


    <!-- http://purl.obolibrary.org/obo/GAZ_00237045 -->

    <owl:NamedIndividual rdf:about="http://purl.obolibrary.org/obo/GAZ_00237045">
        <obo:RO_0001025 rdf:resource="http://purl.obolibrary.org/obo/GAZ_00015501"/>
        <obo:IAO_0000115>A fourth-level administrative division of Uganda.</obo:IAO_0000115>
        <oboInOwl:hasOBONamespace>GAZ</oboInOwl:hasOBONamespace>
        <oboInOwl:id>GAZ:00237045</oboInOwl:id>
        <rdfs:label>Palabek Kal Sub-county</rdfs:label>
    </owl:NamedIndividual>
    


    <!-- http://purl.obolibrary.org/obo/GAZ_00237046 -->

    <owl:NamedIndividual rdf:about="http://purl.obolibrary.org/obo/GAZ_00237046">
        <obo:RO_0001025 rdf:resource="http://purl.obolibrary.org/obo/GAZ_00015501"/>
        <obo:IAO_0000115>A fourth-level administrative division of Uganda.</obo:IAO_0000115>
        <oboInOwl:hasOBONamespace>GAZ</oboInOwl:hasOBONamespace>
        <oboInOwl:id>GAZ:00237046</oboInOwl:id>
        <rdfs:label>Paloga Sub-county</rdfs:label>
    </owl:NamedIndividual>
    


    <!-- http://purl.obolibrary.org/obo/GAZ_00237047 -->

    <owl:NamedIndividual rdf:about="http://purl.obolibrary.org/obo/GAZ_00237047">
        <obo:RO_0001025 rdf:resource="http://purl.obolibrary.org/obo/GAZ_00233545"/>
        <obo:IAO_0000115>A fourth-level administrative division of Uganda.</obo:IAO_0000115>
        <oboInOwl:hasOBONamespace>GAZ</oboInOwl:hasOBONamespace>
        <oboInOwl:id>GAZ:00237047</oboInOwl:id>
        <rdfs:label>Iriiri Sub-county</rdfs:label>
    </owl:NamedIndividual>
    


    <!-- http://purl.obolibrary.org/obo/GAZ_00237048 -->

    <owl:NamedIndividual rdf:about="http://purl.obolibrary.org/obo/GAZ_00237048">
        <obo:RO_0001025 rdf:resource="http://purl.obolibrary.org/obo/GAZ_00233545"/>
        <obo:IAO_0000115>A fourth-level administrative division of Uganda.</obo:IAO_0000115>
        <oboInOwl:hasOBONamespace>GAZ</oboInOwl:hasOBONamespace>
        <oboInOwl:id>GAZ:00237048</oboInOwl:id>
        <rdfs:label>Lokopo Sub-county</rdfs:label>
    </owl:NamedIndividual>
    


    <!-- http://purl.obolibrary.org/obo/GAZ_00237049 -->

    <owl:NamedIndividual rdf:about="http://purl.obolibrary.org/obo/GAZ_00237049">
        <obo:RO_0001025 rdf:resource="http://purl.obolibrary.org/obo/GAZ_00233545"/>
        <obo:IAO_0000115>A fourth-level administrative division of Uganda.</obo:IAO_0000115>
        <oboInOwl:hasOBONamespace>GAZ</oboInOwl:hasOBONamespace>
        <oboInOwl:id>GAZ:00237049</oboInOwl:id>
        <rdfs:label>Lopei Sub-county</rdfs:label>
    </owl:NamedIndividual>
    


    <!-- http://purl.obolibrary.org/obo/GAZ_00237050 -->

    <owl:NamedIndividual rdf:about="http://purl.obolibrary.org/obo/GAZ_00237050">
        <obo:RO_0001025 rdf:resource="http://purl.obolibrary.org/obo/GAZ_00233545"/>
        <obo:IAO_0000115>A fourth-level administrative division of Uganda.</obo:IAO_0000115>
        <oboInOwl:hasOBONamespace>GAZ</oboInOwl:hasOBONamespace>
        <oboInOwl:id>GAZ:00237050</oboInOwl:id>
        <rdfs:label>Lotome Sub-county</rdfs:label>
    </owl:NamedIndividual>
    


    <!-- http://purl.obolibrary.org/obo/GAZ_00237051 -->

    <owl:NamedIndividual rdf:about="http://purl.obolibrary.org/obo/GAZ_00237051">
        <obo:RO_0001025 rdf:resource="http://purl.obolibrary.org/obo/GAZ_00233545"/>
        <obo:IAO_0000115>A fourth-level administrative division of Uganda.</obo:IAO_0000115>
        <oboInOwl:hasOBONamespace>GAZ</oboInOwl:hasOBONamespace>
        <oboInOwl:id>GAZ:00237051</oboInOwl:id>
        <rdfs:label>Matany Sub-county</rdfs:label>
    </owl:NamedIndividual>
    


    <!-- http://purl.obolibrary.org/obo/GAZ_00237052 -->

    <owl:NamedIndividual rdf:about="http://purl.obolibrary.org/obo/GAZ_00237052">
        <obo:RO_0001025 rdf:resource="http://purl.obolibrary.org/obo/GAZ_00233545"/>
        <obo:IAO_0000115>A fourth-level administrative division of Uganda.</obo:IAO_0000115>
        <oboInOwl:hasOBONamespace>GAZ</oboInOwl:hasOBONamespace>
        <oboInOwl:id>GAZ:00237052</oboInOwl:id>
        <rdfs:label>Ngoleriet Sub-county</rdfs:label>
    </owl:NamedIndividual>
    


    <!-- http://purl.obolibrary.org/obo/GAZ_00237053 -->

    <owl:NamedIndividual rdf:about="http://purl.obolibrary.org/obo/GAZ_00237053">
        <obo:RO_0001025 rdf:resource="http://purl.obolibrary.org/obo/GAZ_00233546"/>
        <obo:IAO_0000115>A fourth-level administrative division of Uganda.</obo:IAO_0000115>
        <oboInOwl:hasOBONamespace>GAZ</oboInOwl:hasOBONamespace>
        <oboInOwl:id>GAZ:00237053</oboInOwl:id>
        <rdfs:label>Katikekile Sub-county</rdfs:label>
    </owl:NamedIndividual>
    


    <!-- http://purl.obolibrary.org/obo/GAZ_00237054 -->

    <owl:NamedIndividual rdf:about="http://purl.obolibrary.org/obo/GAZ_00237054">
        <obo:RO_0001025 rdf:resource="http://purl.obolibrary.org/obo/GAZ_00233546"/>
        <obo:IAO_0000115>A fourth-level administrative division of Uganda.</obo:IAO_0000115>
        <oboInOwl:hasOBONamespace>GAZ</oboInOwl:hasOBONamespace>
        <oboInOwl:id>GAZ:00237054</oboInOwl:id>
        <rdfs:label>Nadunget Sub-county</rdfs:label>
    </owl:NamedIndividual>
    


    <!-- http://purl.obolibrary.org/obo/GAZ_00237055 -->

    <owl:NamedIndividual rdf:about="http://purl.obolibrary.org/obo/GAZ_00237055">
        <obo:RO_0001025 rdf:resource="http://purl.obolibrary.org/obo/GAZ_00233546"/>
        <obo:IAO_0000115>A fourth-level administrative division of Uganda.</obo:IAO_0000115>
        <oboInOwl:hasOBONamespace>GAZ</oboInOwl:hasOBONamespace>
        <oboInOwl:id>GAZ:00237055</oboInOwl:id>
        <rdfs:label>Rupa Sub-county</rdfs:label>
    </owl:NamedIndividual>
    


    <!-- http://purl.obolibrary.org/obo/GAZ_00237056 -->

    <owl:NamedIndividual rdf:about="http://purl.obolibrary.org/obo/GAZ_00237056">
        <obo:RO_0001025 rdf:resource="http://purl.obolibrary.org/obo/GAZ_00233547"/>
        <obo:IAO_0000115>A fourth-level administrative division of Uganda.</obo:IAO_0000115>
        <oboInOwl:hasOBONamespace>GAZ</oboInOwl:hasOBONamespace>
        <oboInOwl:id>GAZ:00237056</oboInOwl:id>
        <rdfs:label>Moroto Northern Division</rdfs:label>
    </owl:NamedIndividual>
    


    <!-- http://purl.obolibrary.org/obo/GAZ_00237057 -->

    <owl:NamedIndividual rdf:about="http://purl.obolibrary.org/obo/GAZ_00237057">
        <obo:RO_0001025 rdf:resource="http://purl.obolibrary.org/obo/GAZ_00233547"/>
        <obo:IAO_0000115>A fourth-level administrative division of Uganda.</obo:IAO_0000115>
        <oboInOwl:hasOBONamespace>GAZ</oboInOwl:hasOBONamespace>
        <oboInOwl:id>GAZ:00237057</oboInOwl:id>
        <rdfs:label>Moroto Southern Dovision</rdfs:label>
    </owl:NamedIndividual>
    


    <!-- http://purl.obolibrary.org/obo/GAZ_00237058 -->

    <owl:NamedIndividual rdf:about="http://purl.obolibrary.org/obo/GAZ_00237058">
        <obo:RO_0001025 rdf:resource="http://purl.obolibrary.org/obo/GAZ_00015510"/>
        <obo:IAO_0000115>A fourth-level administrative division of Uganda.</obo:IAO_0000115>
        <oboInOwl:hasOBONamespace>GAZ</oboInOwl:hasOBONamespace>
        <oboInOwl:id>GAZ:00237058</oboInOwl:id>
        <rdfs:label>Aliba Sub-county</rdfs:label>
    </owl:NamedIndividual>
    


    <!-- http://purl.obolibrary.org/obo/GAZ_00237059 -->

    <owl:NamedIndividual rdf:about="http://purl.obolibrary.org/obo/GAZ_00237059">
        <obo:RO_0001025 rdf:resource="http://purl.obolibrary.org/obo/GAZ_00015510"/>
        <obo:IAO_0000115>A fourth-level administrative division of Uganda.</obo:IAO_0000115>
        <oboInOwl:hasOBONamespace>GAZ</oboInOwl:hasOBONamespace>
        <oboInOwl:id>GAZ:00237059</oboInOwl:id>
        <rdfs:label>Gimara Sub-county</rdfs:label>
    </owl:NamedIndividual>
    


    <!-- http://purl.obolibrary.org/obo/GAZ_00237060 -->

    <owl:NamedIndividual rdf:about="http://purl.obolibrary.org/obo/GAZ_00237060">
        <obo:RO_0001025 rdf:resource="http://purl.obolibrary.org/obo/GAZ_00015510"/>
        <obo:IAO_0000115>A fourth-level administrative division of Uganda.</obo:IAO_0000115>
        <oboInOwl:hasOBONamespace>GAZ</oboInOwl:hasOBONamespace>
        <oboInOwl:id>GAZ:00237060</oboInOwl:id>
        <rdfs:label>Itula Sub-county</rdfs:label>
    </owl:NamedIndividual>
    


    <!-- http://purl.obolibrary.org/obo/GAZ_00237061 -->

    <owl:NamedIndividual rdf:about="http://purl.obolibrary.org/obo/GAZ_00237061">
        <obo:RO_0001025 rdf:resource="http://purl.obolibrary.org/obo/GAZ_00015511"/>
        <obo:IAO_0000115>A fourth-level administrative division of Uganda.</obo:IAO_0000115>
        <oboInOwl:hasOBONamespace>GAZ</oboInOwl:hasOBONamespace>
        <oboInOwl:id>GAZ:00237061</oboInOwl:id>
        <rdfs:label>Dufile Sub-county</rdfs:label>
    </owl:NamedIndividual>
    


    <!-- http://purl.obolibrary.org/obo/GAZ_00237062 -->

    <owl:NamedIndividual rdf:about="http://purl.obolibrary.org/obo/GAZ_00237062">
        <obo:RO_0001025 rdf:resource="http://purl.obolibrary.org/obo/GAZ_00015511"/>
        <obo:IAO_0000115>A fourth-level administrative division of Uganda.</obo:IAO_0000115>
        <oboInOwl:hasOBONamespace>GAZ</oboInOwl:hasOBONamespace>
        <oboInOwl:id>GAZ:00237062</oboInOwl:id>
        <rdfs:label>Lefori Sub-county</rdfs:label>
    </owl:NamedIndividual>
    


    <!-- http://purl.obolibrary.org/obo/GAZ_00237063 -->

    <owl:NamedIndividual rdf:about="http://purl.obolibrary.org/obo/GAZ_00237063">
        <obo:RO_0001025 rdf:resource="http://purl.obolibrary.org/obo/GAZ_00015511"/>
        <obo:IAO_0000115>A fourth-level administrative division of Uganda.</obo:IAO_0000115>
        <oboInOwl:hasOBONamespace>GAZ</oboInOwl:hasOBONamespace>
        <oboInOwl:id>GAZ:00237063</oboInOwl:id>
        <rdfs:label>Metu Sub-county</rdfs:label>
    </owl:NamedIndividual>
    


    <!-- http://purl.obolibrary.org/obo/GAZ_00237064 -->

    <owl:NamedIndividual rdf:about="http://purl.obolibrary.org/obo/GAZ_00237064">
        <obo:RO_0001025 rdf:resource="http://purl.obolibrary.org/obo/GAZ_00015511"/>
        <obo:IAO_0000115>A fourth-level administrative division of Uganda.</obo:IAO_0000115>
        <oboInOwl:hasOBONamespace>GAZ</oboInOwl:hasOBONamespace>
        <oboInOwl:id>GAZ:00237064</oboInOwl:id>
        <rdfs:label>Moyo Town</rdfs:label>
    </owl:NamedIndividual>
    


    <!-- http://purl.obolibrary.org/obo/GAZ_00237065 -->

    <owl:NamedIndividual rdf:about="http://purl.obolibrary.org/obo/GAZ_00237065">
        <obo:RO_0001025 rdf:resource="http://purl.obolibrary.org/obo/GAZ_00015511"/>
        <obo:IAO_0000115>A fourth-level administrative division of Uganda.</obo:IAO_0000115>
        <oboInOwl:hasOBONamespace>GAZ</oboInOwl:hasOBONamespace>
        <oboInOwl:id>GAZ:00237065</oboInOwl:id>
        <rdfs:label>Moyo Sub-county</rdfs:label>
    </owl:NamedIndividual>
    


    <!-- http://purl.obolibrary.org/obo/GAZ_00237066 -->

    <owl:NamedIndividual rdf:about="http://purl.obolibrary.org/obo/GAZ_00237066">
        <obo:RO_0001025 rdf:resource="http://purl.obolibrary.org/obo/GAZ_00015515"/>
        <obo:IAO_0000115>A fourth-level administrative division of Uganda.</obo:IAO_0000115>
        <oboInOwl:hasOBONamespace>GAZ</oboInOwl:hasOBONamespace>
        <oboInOwl:id>GAZ:00237066</oboInOwl:id>
        <rdfs:label>Pakwach Sub-county</rdfs:label>
    </owl:NamedIndividual>
    


    <!-- http://purl.obolibrary.org/obo/GAZ_00237067 -->

    <owl:NamedIndividual rdf:about="http://purl.obolibrary.org/obo/GAZ_00237067">
        <obo:RO_0001025 rdf:resource="http://purl.obolibrary.org/obo/GAZ_00015515"/>
        <obo:IAO_0000115>A fourth-level administrative division of Uganda.</obo:IAO_0000115>
        <oboInOwl:hasOBONamespace>GAZ</oboInOwl:hasOBONamespace>
        <oboInOwl:id>GAZ:00237067</oboInOwl:id>
        <rdfs:label>Pakwach Town</rdfs:label>
    </owl:NamedIndividual>
    


    <!-- http://purl.obolibrary.org/obo/GAZ_00237068 -->

    <owl:NamedIndividual rdf:about="http://purl.obolibrary.org/obo/GAZ_00237068">
        <obo:RO_0001025 rdf:resource="http://purl.obolibrary.org/obo/GAZ_00015515"/>
        <obo:IAO_0000115>A fourth-level administrative division of Uganda.</obo:IAO_0000115>
        <oboInOwl:hasOBONamespace>GAZ</oboInOwl:hasOBONamespace>
        <oboInOwl:id>GAZ:00237068</oboInOwl:id>
        <rdfs:label>Panyango Sub-county</rdfs:label>
    </owl:NamedIndividual>
    


    <!-- http://purl.obolibrary.org/obo/GAZ_00237069 -->

    <owl:NamedIndividual rdf:about="http://purl.obolibrary.org/obo/GAZ_00237069">
        <obo:RO_0001025 rdf:resource="http://purl.obolibrary.org/obo/GAZ_00015515"/>
        <obo:IAO_0000115>A fourth-level administrative division of Uganda.</obo:IAO_0000115>
        <oboInOwl:hasOBONamespace>GAZ</oboInOwl:hasOBONamespace>
        <oboInOwl:id>GAZ:00237069</oboInOwl:id>
        <rdfs:label>Panyimur Sub-county</rdfs:label>
    </owl:NamedIndividual>
    


    <!-- http://purl.obolibrary.org/obo/GAZ_00237070 -->

    <owl:NamedIndividual rdf:about="http://purl.obolibrary.org/obo/GAZ_00237070">
        <obo:RO_0001025 rdf:resource="http://purl.obolibrary.org/obo/GAZ_00015515"/>
        <obo:IAO_0000115>A fourth-level administrative division of Uganda.</obo:IAO_0000115>
        <oboInOwl:hasOBONamespace>GAZ</oboInOwl:hasOBONamespace>
        <oboInOwl:id>GAZ:00237070</oboInOwl:id>
        <rdfs:label>Wadelai Sub-county</rdfs:label>
    </owl:NamedIndividual>
    


    <!-- http://purl.obolibrary.org/obo/GAZ_00237071 -->

    <owl:NamedIndividual rdf:about="http://purl.obolibrary.org/obo/GAZ_00237071">
        <obo:RO_0001025 rdf:resource="http://purl.obolibrary.org/obo/GAZ_00015514"/>
        <obo:IAO_0000115>A fourth-level administrative division of Uganda.</obo:IAO_0000115>
        <oboInOwl:hasOBONamespace>GAZ</oboInOwl:hasOBONamespace>
        <oboInOwl:id>GAZ:00237071</oboInOwl:id>
        <rdfs:label>Atyak Sub-county</rdfs:label>
    </owl:NamedIndividual>
    


    <!-- http://purl.obolibrary.org/obo/GAZ_00237072 -->

    <owl:NamedIndividual rdf:about="http://purl.obolibrary.org/obo/GAZ_00237072">
        <obo:RO_0001025 rdf:resource="http://purl.obolibrary.org/obo/GAZ_00015514"/>
        <obo:IAO_0000115>A fourth-level administrative division of Uganda.</obo:IAO_0000115>
        <oboInOwl:hasOBONamespace>GAZ</oboInOwl:hasOBONamespace>
        <oboInOwl:id>GAZ:00237072</oboInOwl:id>
        <rdfs:label>Jangokoro Sub-county</rdfs:label>
    </owl:NamedIndividual>
    


    <!-- http://purl.obolibrary.org/obo/GAZ_00237073 -->

    <owl:NamedIndividual rdf:about="http://purl.obolibrary.org/obo/GAZ_00237073">
        <obo:RO_0001025 rdf:resource="http://purl.obolibrary.org/obo/GAZ_00015514"/>
        <obo:IAO_0000115>A fourth-level administrative division of Uganda.</obo:IAO_0000115>
        <oboInOwl:hasOBONamespace>GAZ</oboInOwl:hasOBONamespace>
        <oboInOwl:id>GAZ:00237073</oboInOwl:id>
        <rdfs:label>Kango Sub-county</rdfs:label>
    </owl:NamedIndividual>
    


    <!-- http://purl.obolibrary.org/obo/GAZ_00237074 -->

    <owl:NamedIndividual rdf:about="http://purl.obolibrary.org/obo/GAZ_00237074">
        <obo:RO_0001025 rdf:resource="http://purl.obolibrary.org/obo/GAZ_00015514"/>
        <obo:IAO_0000115>A fourth-level administrative division of Uganda.</obo:IAO_0000115>
        <oboInOwl:hasOBONamespace>GAZ</oboInOwl:hasOBONamespace>
        <oboInOwl:id>GAZ:00237074</oboInOwl:id>
        <rdfs:label>Nyapea Sub-county</rdfs:label>
    </owl:NamedIndividual>
    


    <!-- http://purl.obolibrary.org/obo/GAZ_00237075 -->

    <owl:NamedIndividual rdf:about="http://purl.obolibrary.org/obo/GAZ_00237075">
        <obo:RO_0001025 rdf:resource="http://purl.obolibrary.org/obo/GAZ_00015514"/>
        <obo:IAO_0000115>A fourth-level administrative division of Uganda.</obo:IAO_0000115>
        <oboInOwl:hasOBONamespace>GAZ</oboInOwl:hasOBONamespace>
        <oboInOwl:id>GAZ:00237075</oboInOwl:id>
        <rdfs:label>Paidha Sub-county</rdfs:label>
    </owl:NamedIndividual>
    


    <!-- http://purl.obolibrary.org/obo/GAZ_00237076 -->

    <owl:NamedIndividual rdf:about="http://purl.obolibrary.org/obo/GAZ_00237076">
        <obo:RO_0001025 rdf:resource="http://purl.obolibrary.org/obo/GAZ_00015514"/>
        <obo:IAO_0000115>A fourth-level administrative division of Uganda.</obo:IAO_0000115>
        <oboInOwl:hasOBONamespace>GAZ</oboInOwl:hasOBONamespace>
        <oboInOwl:id>GAZ:00237076</oboInOwl:id>
        <rdfs:label>Paidha Town</rdfs:label>
    </owl:NamedIndividual>
    


    <!-- http://purl.obolibrary.org/obo/GAZ_00237077 -->

    <owl:NamedIndividual rdf:about="http://purl.obolibrary.org/obo/GAZ_00237077">
        <obo:RO_0001025 rdf:resource="http://purl.obolibrary.org/obo/GAZ_00015514"/>
        <obo:IAO_0000115>A fourth-level administrative division of Uganda.</obo:IAO_0000115>
        <oboInOwl:hasOBONamespace>GAZ</oboInOwl:hasOBONamespace>
        <oboInOwl:id>GAZ:00237077</oboInOwl:id>
        <rdfs:label>Zeu Sub-county</rdfs:label>
    </owl:NamedIndividual>
    


    <!-- http://purl.obolibrary.org/obo/GAZ_00237078 -->

    <owl:NamedIndividual rdf:about="http://purl.obolibrary.org/obo/GAZ_00237078">
        <obo:RO_0001025 rdf:resource="http://purl.obolibrary.org/obo/GAZ_00015516"/>
        <obo:IAO_0000115>A fourth-level administrative division of Uganda.</obo:IAO_0000115>
        <oboInOwl:hasOBONamespace>GAZ</oboInOwl:hasOBONamespace>
        <oboInOwl:id>GAZ:00237078</oboInOwl:id>
        <rdfs:label>Akworo Sub-county</rdfs:label>
    </owl:NamedIndividual>
    


    <!-- http://purl.obolibrary.org/obo/GAZ_00237079 -->

    <owl:NamedIndividual rdf:about="http://purl.obolibrary.org/obo/GAZ_00237079">
        <obo:RO_0001025 rdf:resource="http://purl.obolibrary.org/obo/GAZ_00015516"/>
        <obo:IAO_0000115>A fourth-level administrative division of Uganda.</obo:IAO_0000115>
        <oboInOwl:hasOBONamespace>GAZ</oboInOwl:hasOBONamespace>
        <oboInOwl:id>GAZ:00237079</oboInOwl:id>
        <rdfs:label>Erussi Sub-county</rdfs:label>
    </owl:NamedIndividual>
    


    <!-- http://purl.obolibrary.org/obo/GAZ_00237080 -->

    <owl:NamedIndividual rdf:about="http://purl.obolibrary.org/obo/GAZ_00237080">
        <obo:RO_0001025 rdf:resource="http://purl.obolibrary.org/obo/GAZ_00015516"/>
        <obo:IAO_0000115>A fourth-level administrative division of Uganda.</obo:IAO_0000115>
        <oboInOwl:hasOBONamespace>GAZ</oboInOwl:hasOBONamespace>
        <oboInOwl:id>GAZ:00237080</oboInOwl:id>
        <rdfs:label>Kucwiny Sub-county</rdfs:label>
    </owl:NamedIndividual>
    


    <!-- http://purl.obolibrary.org/obo/GAZ_00237081 -->

    <owl:NamedIndividual rdf:about="http://purl.obolibrary.org/obo/GAZ_00237081">
        <obo:RO_0001025 rdf:resource="http://purl.obolibrary.org/obo/GAZ_00015516"/>
        <obo:IAO_0000115>A fourth-level administrative division of Uganda.</obo:IAO_0000115>
        <oboInOwl:hasOBONamespace>GAZ</oboInOwl:hasOBONamespace>
        <oboInOwl:id>GAZ:00237081</oboInOwl:id>
        <rdfs:label>Nebbi Sub-county</rdfs:label>
    </owl:NamedIndividual>
    


    <!-- http://purl.obolibrary.org/obo/GAZ_00237082 -->

    <owl:NamedIndividual rdf:about="http://purl.obolibrary.org/obo/GAZ_00237082">
        <obo:RO_0001025 rdf:resource="http://purl.obolibrary.org/obo/GAZ_00015516"/>
        <obo:IAO_0000115>A fourth-level administrative division of Uganda.</obo:IAO_0000115>
        <oboInOwl:hasOBONamespace>GAZ</oboInOwl:hasOBONamespace>
        <oboInOwl:id>GAZ:00237082</oboInOwl:id>
        <rdfs:label>Nebbi Town</rdfs:label>
    </owl:NamedIndividual>
    


    <!-- http://purl.obolibrary.org/obo/GAZ_00237083 -->

    <owl:NamedIndividual rdf:about="http://purl.obolibrary.org/obo/GAZ_00237083">
        <obo:RO_0001025 rdf:resource="http://purl.obolibrary.org/obo/GAZ_00015516"/>
        <obo:IAO_0000115>A fourth-level administrative division of Uganda.</obo:IAO_0000115>
        <oboInOwl:hasOBONamespace>GAZ</oboInOwl:hasOBONamespace>
        <oboInOwl:id>GAZ:00237083</oboInOwl:id>
        <rdfs:label>Nyaravur Sub-county</rdfs:label>
    </owl:NamedIndividual>
    


    <!-- http://purl.obolibrary.org/obo/GAZ_00237084 -->

    <owl:NamedIndividual rdf:about="http://purl.obolibrary.org/obo/GAZ_00237084">
        <obo:RO_0001025 rdf:resource="http://purl.obolibrary.org/obo/GAZ_00015516"/>
        <obo:IAO_0000115>A fourth-level administrative division of Uganda.</obo:IAO_0000115>
        <oboInOwl:hasOBONamespace>GAZ</oboInOwl:hasOBONamespace>
        <oboInOwl:id>GAZ:00237084</oboInOwl:id>
        <rdfs:label>Parombo Sub-county</rdfs:label>
    </owl:NamedIndividual>
    


    <!-- http://purl.obolibrary.org/obo/GAZ_00237085 -->

    <owl:NamedIndividual rdf:about="http://purl.obolibrary.org/obo/GAZ_00237085">
        <obo:RO_0001025 rdf:resource="http://purl.obolibrary.org/obo/GAZ_00015512"/>
        <obo:IAO_0000115>A fourth-level administrative division of Uganda.</obo:IAO_0000115>
        <oboInOwl:hasOBONamespace>GAZ</oboInOwl:hasOBONamespace>
        <oboInOwl:id>GAZ:00237085</oboInOwl:id>
        <rdfs:label>Kakomongole Sub-county</rdfs:label>
    </owl:NamedIndividual>
    


    <!-- http://purl.obolibrary.org/obo/GAZ_00237086 -->

    <owl:NamedIndividual rdf:about="http://purl.obolibrary.org/obo/GAZ_00237086">
        <obo:RO_0001025 rdf:resource="http://purl.obolibrary.org/obo/GAZ_00015512"/>
        <obo:IAO_0000115>A fourth-level administrative division of Uganda.</obo:IAO_0000115>
        <oboInOwl:hasOBONamespace>GAZ</oboInOwl:hasOBONamespace>
        <oboInOwl:id>GAZ:00237086</oboInOwl:id>
        <rdfs:label>Moruita Sub-county</rdfs:label>
    </owl:NamedIndividual>
    


    <!-- http://purl.obolibrary.org/obo/GAZ_00237087 -->

    <owl:NamedIndividual rdf:about="http://purl.obolibrary.org/obo/GAZ_00237087">
        <obo:RO_0001025 rdf:resource="http://purl.obolibrary.org/obo/GAZ_00015512"/>
        <obo:IAO_0000115>A fourth-level administrative division of Uganda.</obo:IAO_0000115>
        <oboInOwl:hasOBONamespace>GAZ</oboInOwl:hasOBONamespace>
        <oboInOwl:id>GAZ:00237087</oboInOwl:id>
        <rdfs:label>Nakapiripirit Town</rdfs:label>
    </owl:NamedIndividual>
    


    <!-- http://purl.obolibrary.org/obo/GAZ_00237088 -->

    <owl:NamedIndividual rdf:about="http://purl.obolibrary.org/obo/GAZ_00237088">
        <obo:RO_0001025 rdf:resource="http://purl.obolibrary.org/obo/GAZ_00015512"/>
        <obo:IAO_0000115>A fourth-level administrative division of Uganda.</obo:IAO_0000115>
        <oboInOwl:hasOBONamespace>GAZ</oboInOwl:hasOBONamespace>
        <oboInOwl:id>GAZ:00237088</oboInOwl:id>
        <rdfs:label>Namalu Sub-county</rdfs:label>
    </owl:NamedIndividual>
    


    <!-- http://purl.obolibrary.org/obo/GAZ_00237089 -->

    <owl:NamedIndividual rdf:about="http://purl.obolibrary.org/obo/GAZ_00237089">
        <obo:RO_0001025 rdf:resource="http://purl.obolibrary.org/obo/GAZ_00015513"/>
        <obo:IAO_0000115>A fourth-level administrative division of Uganda.</obo:IAO_0000115>
        <oboInOwl:hasOBONamespace>GAZ</oboInOwl:hasOBONamespace>
        <oboInOwl:id>GAZ:00237089</oboInOwl:id>
        <rdfs:label>Lolachat Sub-county</rdfs:label>
    </owl:NamedIndividual>
    


    <!-- http://purl.obolibrary.org/obo/GAZ_00237090 -->

    <owl:NamedIndividual rdf:about="http://purl.obolibrary.org/obo/GAZ_00237090">
        <obo:RO_0001025 rdf:resource="http://purl.obolibrary.org/obo/GAZ_00015513"/>
        <obo:IAO_0000115>A fourth-level administrative division of Uganda.</obo:IAO_0000115>
        <oboInOwl:hasOBONamespace>GAZ</oboInOwl:hasOBONamespace>
        <oboInOwl:id>GAZ:00237090</oboInOwl:id>
        <rdfs:label>Lorengedwat Sub-county</rdfs:label>
    </owl:NamedIndividual>
    


    <!-- http://purl.obolibrary.org/obo/GAZ_00237091 -->

    <owl:NamedIndividual rdf:about="http://purl.obolibrary.org/obo/GAZ_00237091">
        <obo:RO_0001025 rdf:resource="http://purl.obolibrary.org/obo/GAZ_00015513"/>
        <obo:IAO_0000115>A fourth-level administrative division of Uganda.</obo:IAO_0000115>
        <oboInOwl:hasOBONamespace>GAZ</oboInOwl:hasOBONamespace>
        <oboInOwl:id>GAZ:00237091</oboInOwl:id>
        <rdfs:label>Nabilatuk Sub-county</rdfs:label>
    </owl:NamedIndividual>
    


    <!-- http://purl.obolibrary.org/obo/GAZ_00237092 -->

    <owl:NamedIndividual rdf:about="http://purl.obolibrary.org/obo/GAZ_00237092">
        <obo:RO_0001025 rdf:resource="http://purl.obolibrary.org/obo/GAZ_00015517"/>
        <obo:IAO_0000115>A fourth-level administrative division of Uganda.</obo:IAO_0000115>
        <oboInOwl:hasOBONamespace>GAZ</oboInOwl:hasOBONamespace>
        <oboInOwl:id>GAZ:00237092</oboInOwl:id>
        <rdfs:label>Aber Sub-county</rdfs:label>
    </owl:NamedIndividual>
    


    <!-- http://purl.obolibrary.org/obo/GAZ_00237093 -->

    <owl:NamedIndividual rdf:about="http://purl.obolibrary.org/obo/GAZ_00237093">
        <obo:RO_0001025 rdf:resource="http://purl.obolibrary.org/obo/GAZ_00015517"/>
        <obo:IAO_0000115>A fourth-level administrative division of Uganda.</obo:IAO_0000115>
        <oboInOwl:hasOBONamespace>GAZ</oboInOwl:hasOBONamespace>
        <oboInOwl:id>GAZ:00237093</oboInOwl:id>
        <rdfs:label>Acaba Sub-county</rdfs:label>
    </owl:NamedIndividual>
    


    <!-- http://purl.obolibrary.org/obo/GAZ_00237094 -->

    <owl:NamedIndividual rdf:about="http://purl.obolibrary.org/obo/GAZ_00237094">
        <obo:RO_0001025 rdf:resource="http://purl.obolibrary.org/obo/GAZ_00015517"/>
        <obo:IAO_0000115>A fourth-level administrative division of Uganda.</obo:IAO_0000115>
        <oboInOwl:hasOBONamespace>GAZ</oboInOwl:hasOBONamespace>
        <oboInOwl:id>GAZ:00237094</oboInOwl:id>
        <rdfs:label>Iceme Sub-county</rdfs:label>
    </owl:NamedIndividual>
    


    <!-- http://purl.obolibrary.org/obo/GAZ_00237095 -->

    <owl:NamedIndividual rdf:about="http://purl.obolibrary.org/obo/GAZ_00237095">
        <obo:RO_0001025 rdf:resource="http://purl.obolibrary.org/obo/GAZ_00015517"/>
        <obo:IAO_0000115>A fourth-level administrative division of Uganda.</obo:IAO_0000115>
        <oboInOwl:hasOBONamespace>GAZ</oboInOwl:hasOBONamespace>
        <oboInOwl:id>GAZ:00237095</oboInOwl:id>
        <rdfs:label>Loro Sub-county</rdfs:label>
    </owl:NamedIndividual>
    


    <!-- http://purl.obolibrary.org/obo/GAZ_00237096 -->

    <owl:NamedIndividual rdf:about="http://purl.obolibrary.org/obo/GAZ_00237096">
        <obo:RO_0001025 rdf:resource="http://purl.obolibrary.org/obo/GAZ_00015517"/>
        <obo:IAO_0000115>A fourth-level administrative division of Uganda.</obo:IAO_0000115>
        <oboInOwl:hasOBONamespace>GAZ</oboInOwl:hasOBONamespace>
        <oboInOwl:id>GAZ:00237096</oboInOwl:id>
        <rdfs:label>Minakulu Sub-county</rdfs:label>
    </owl:NamedIndividual>
    


    <!-- http://purl.obolibrary.org/obo/GAZ_00237097 -->

    <owl:NamedIndividual rdf:about="http://purl.obolibrary.org/obo/GAZ_00237097">
        <obo:RO_0001025 rdf:resource="http://purl.obolibrary.org/obo/GAZ_00015517"/>
        <obo:IAO_0000115>A fourth-level administrative division of Uganda.</obo:IAO_0000115>
        <oboInOwl:hasOBONamespace>GAZ</oboInOwl:hasOBONamespace>
        <oboInOwl:id>GAZ:00237097</oboInOwl:id>
        <rdfs:label>Ngai Sub-county</rdfs:label>
    </owl:NamedIndividual>
    


    <!-- http://purl.obolibrary.org/obo/GAZ_00237098 -->

    <owl:NamedIndividual rdf:about="http://purl.obolibrary.org/obo/GAZ_00237098">
        <obo:RO_0001025 rdf:resource="http://purl.obolibrary.org/obo/GAZ_00015517"/>
        <obo:IAO_0000115>A fourth-level administrative division of Uganda.</obo:IAO_0000115>
        <oboInOwl:hasOBONamespace>GAZ</oboInOwl:hasOBONamespace>
        <oboInOwl:id>GAZ:00237098</oboInOwl:id>
        <rdfs:label>Otwal Sub-county</rdfs:label>
    </owl:NamedIndividual>
    


    <!-- http://purl.obolibrary.org/obo/GAZ_00237099 -->

    <owl:NamedIndividual rdf:about="http://purl.obolibrary.org/obo/GAZ_00237099">
        <obo:RO_0001025 rdf:resource="http://purl.obolibrary.org/obo/GAZ_00015518"/>
        <obo:IAO_0000115>A fourth-level administrative division of Uganda.</obo:IAO_0000115>
        <oboInOwl:hasOBONamespace>GAZ</oboInOwl:hasOBONamespace>
        <oboInOwl:id>GAZ:00237099</oboInOwl:id>
        <rdfs:label>Adilang Sub-county</rdfs:label>
    </owl:NamedIndividual>
    


    <!-- http://purl.obolibrary.org/obo/GAZ_00237100 -->

    <owl:NamedIndividual rdf:about="http://purl.obolibrary.org/obo/GAZ_00237100">
        <obo:RO_0001025 rdf:resource="http://purl.obolibrary.org/obo/GAZ_00015518"/>
        <obo:IAO_0000115>A fourth-level administrative division of Uganda.</obo:IAO_0000115>
        <oboInOwl:hasOBONamespace>GAZ</oboInOwl:hasOBONamespace>
        <oboInOwl:id>GAZ:00237100</oboInOwl:id>
        <rdfs:label>Lapono Sub-county</rdfs:label>
    </owl:NamedIndividual>
    


    <!-- http://purl.obolibrary.org/obo/GAZ_00237101 -->

    <owl:NamedIndividual rdf:about="http://purl.obolibrary.org/obo/GAZ_00237101">
        <obo:RO_0001025 rdf:resource="http://purl.obolibrary.org/obo/GAZ_00015518"/>
        <obo:IAO_0000115>A fourth-level administrative division of Uganda.</obo:IAO_0000115>
        <oboInOwl:hasOBONamespace>GAZ</oboInOwl:hasOBONamespace>
        <oboInOwl:id>GAZ:00237101</oboInOwl:id>
        <rdfs:label>Lira Palwo Sub-county</rdfs:label>
    </owl:NamedIndividual>
    


    <!-- http://purl.obolibrary.org/obo/GAZ_00237102 -->

    <owl:NamedIndividual rdf:about="http://purl.obolibrary.org/obo/GAZ_00237102">
        <obo:RO_0001025 rdf:resource="http://purl.obolibrary.org/obo/GAZ_00015518"/>
        <obo:IAO_0000115>A fourth-level administrative division of Uganda.</obo:IAO_0000115>
        <oboInOwl:hasOBONamespace>GAZ</oboInOwl:hasOBONamespace>
        <oboInOwl:id>GAZ:00237102</oboInOwl:id>
        <rdfs:label>Lukole Sub-county</rdfs:label>
    </owl:NamedIndividual>
    


    <!-- http://purl.obolibrary.org/obo/GAZ_00237103 -->

    <owl:NamedIndividual rdf:about="http://purl.obolibrary.org/obo/GAZ_00237103">
        <obo:RO_0001025 rdf:resource="http://purl.obolibrary.org/obo/GAZ_00015518"/>
        <obo:IAO_0000115>A fourth-level administrative division of Uganda.</obo:IAO_0000115>
        <oboInOwl:hasOBONamespace>GAZ</oboInOwl:hasOBONamespace>
        <oboInOwl:id>GAZ:00237103</oboInOwl:id>
        <rdfs:label>Omot Sub-county</rdfs:label>
    </owl:NamedIndividual>
    


    <!-- http://purl.obolibrary.org/obo/GAZ_00237104 -->

    <owl:NamedIndividual rdf:about="http://purl.obolibrary.org/obo/GAZ_00237104">
        <obo:RO_0001025 rdf:resource="http://purl.obolibrary.org/obo/GAZ_00015518"/>
        <obo:IAO_0000115>A fourth-level administrative division of Uganda.</obo:IAO_0000115>
        <oboInOwl:hasOBONamespace>GAZ</oboInOwl:hasOBONamespace>
        <oboInOwl:id>GAZ:00237104</oboInOwl:id>
        <rdfs:label>Paimol Sub-county</rdfs:label>
    </owl:NamedIndividual>
    


    <!-- http://purl.obolibrary.org/obo/GAZ_00237105 -->

    <owl:NamedIndividual rdf:about="http://purl.obolibrary.org/obo/GAZ_00237105">
        <obo:RO_0001025 rdf:resource="http://purl.obolibrary.org/obo/GAZ_00015518"/>
        <obo:IAO_0000115>A fourth-level administrative division of Uganda.</obo:IAO_0000115>
        <oboInOwl:hasOBONamespace>GAZ</oboInOwl:hasOBONamespace>
        <oboInOwl:id>GAZ:00237105</oboInOwl:id>
        <rdfs:label>Parabongo Sub-county</rdfs:label>
    </owl:NamedIndividual>
    


    <!-- http://purl.obolibrary.org/obo/GAZ_00237106 -->

    <owl:NamedIndividual rdf:about="http://purl.obolibrary.org/obo/GAZ_00237106">
        <obo:RO_0001025 rdf:resource="http://purl.obolibrary.org/obo/GAZ_00015518"/>
        <obo:IAO_0000115>A fourth-level administrative division of Uganda.</obo:IAO_0000115>
        <oboInOwl:hasOBONamespace>GAZ</oboInOwl:hasOBONamespace>
        <oboInOwl:id>GAZ:00237106</oboInOwl:id>
        <rdfs:label>Patongo Sub-county</rdfs:label>
    </owl:NamedIndividual>
    


    <!-- http://purl.obolibrary.org/obo/GAZ_00237107 -->

    <owl:NamedIndividual rdf:about="http://purl.obolibrary.org/obo/GAZ_00237107">
        <obo:RO_0001025 rdf:resource="http://purl.obolibrary.org/obo/GAZ_00015518"/>
        <obo:IAO_0000115>A fourth-level administrative division of Uganda.</obo:IAO_0000115>
        <oboInOwl:hasOBONamespace>GAZ</oboInOwl:hasOBONamespace>
        <oboInOwl:id>GAZ:00237107</oboInOwl:id>
        <rdfs:label>Wol Sub-county</rdfs:label>
    </owl:NamedIndividual>
    


    <!-- http://purl.obolibrary.org/obo/GAZ_00237108 -->

    <owl:NamedIndividual rdf:about="http://purl.obolibrary.org/obo/GAZ_00237108">
        <obo:RO_0001025 rdf:resource="http://purl.obolibrary.org/obo/GAZ_00015519"/>
        <obo:IAO_0000115>A fourth-level administrative division of Uganda.</obo:IAO_0000115>
        <oboInOwl:hasOBONamespace>GAZ</oboInOwl:hasOBONamespace>
        <oboInOwl:id>GAZ:00237108</oboInOwl:id>
        <rdfs:label>Acholibur Sub-county</rdfs:label>
    </owl:NamedIndividual>
    


    <!-- http://purl.obolibrary.org/obo/GAZ_00237109 -->

    <owl:NamedIndividual rdf:about="http://purl.obolibrary.org/obo/GAZ_00237109">
        <obo:RO_0001025 rdf:resource="http://purl.obolibrary.org/obo/GAZ_00015519"/>
        <obo:IAO_0000115>A fourth-level administrative division of Uganda.</obo:IAO_0000115>
        <oboInOwl:hasOBONamespace>GAZ</oboInOwl:hasOBONamespace>
        <oboInOwl:id>GAZ:00237109</oboInOwl:id>
        <rdfs:label>Atanga Sub-county</rdfs:label>
    </owl:NamedIndividual>
    


    <!-- http://purl.obolibrary.org/obo/GAZ_00237110 -->

    <owl:NamedIndividual rdf:about="http://purl.obolibrary.org/obo/GAZ_00237110">
        <obo:RO_0001025 rdf:resource="http://purl.obolibrary.org/obo/GAZ_00015519"/>
        <obo:IAO_0000115>A fourth-level administrative division of Uganda.</obo:IAO_0000115>
        <oboInOwl:hasOBONamespace>GAZ</oboInOwl:hasOBONamespace>
        <oboInOwl:id>GAZ:00237110</oboInOwl:id>
        <rdfs:label>Awer Sub-county</rdfs:label>
    </owl:NamedIndividual>
    


    <!-- http://purl.obolibrary.org/obo/GAZ_00237111 -->

    <owl:NamedIndividual rdf:about="http://purl.obolibrary.org/obo/GAZ_00237111">
        <obo:RO_0001025 rdf:resource="http://purl.obolibrary.org/obo/GAZ_00015519"/>
        <obo:IAO_0000115>A fourth-level administrative division of Uganda.</obo:IAO_0000115>
        <oboInOwl:hasOBONamespace>GAZ</oboInOwl:hasOBONamespace>
        <oboInOwl:id>GAZ:00237111</oboInOwl:id>
        <rdfs:label>Kilak Sub-county</rdfs:label>
    </owl:NamedIndividual>
    


    <!-- http://purl.obolibrary.org/obo/GAZ_00237112 -->

    <owl:NamedIndividual rdf:about="http://purl.obolibrary.org/obo/GAZ_00237112">
        <obo:RO_0001025 rdf:resource="http://purl.obolibrary.org/obo/GAZ_00015519"/>
        <obo:IAO_0000115>A fourth-level administrative division of Uganda.</obo:IAO_0000115>
        <oboInOwl:hasOBONamespace>GAZ</oboInOwl:hasOBONamespace>
        <oboInOwl:id>GAZ:00237112</oboInOwl:id>
        <rdfs:label>Laguti Sub-county</rdfs:label>
    </owl:NamedIndividual>
    


    <!-- http://purl.obolibrary.org/obo/GAZ_00237113 -->

    <owl:NamedIndividual rdf:about="http://purl.obolibrary.org/obo/GAZ_00237113">
        <obo:RO_0001025 rdf:resource="http://purl.obolibrary.org/obo/GAZ_00015519"/>
        <obo:IAO_0000115>A fourth-level administrative division of Uganda.</obo:IAO_0000115>
        <oboInOwl:hasOBONamespace>GAZ</oboInOwl:hasOBONamespace>
        <oboInOwl:id>GAZ:00237113</oboInOwl:id>
        <rdfs:label>Lapul Sub-county</rdfs:label>
    </owl:NamedIndividual>
    


    <!-- http://purl.obolibrary.org/obo/GAZ_00237114 -->

    <owl:NamedIndividual rdf:about="http://purl.obolibrary.org/obo/GAZ_00237114">
        <obo:RO_0001025 rdf:resource="http://purl.obolibrary.org/obo/GAZ_00015519"/>
        <obo:IAO_0000115>A fourth-level administrative division of Uganda.</obo:IAO_0000115>
        <oboInOwl:hasOBONamespace>GAZ</oboInOwl:hasOBONamespace>
        <oboInOwl:id>GAZ:00237114</oboInOwl:id>
        <rdfs:label>Pader Town</rdfs:label>
    </owl:NamedIndividual>
    


    <!-- http://purl.obolibrary.org/obo/GAZ_00237115 -->

    <owl:NamedIndividual rdf:about="http://purl.obolibrary.org/obo/GAZ_00237115">
        <obo:RO_0001025 rdf:resource="http://purl.obolibrary.org/obo/GAZ_00015519"/>
        <obo:IAO_0000115>A fourth-level administrative division of Uganda.</obo:IAO_0000115>
        <oboInOwl:hasOBONamespace>GAZ</oboInOwl:hasOBONamespace>
        <oboInOwl:id>GAZ:00237115</oboInOwl:id>
        <rdfs:label>Pajule Sub-county</rdfs:label>
    </owl:NamedIndividual>
    


    <!-- http://purl.obolibrary.org/obo/GAZ_00237116 -->

    <owl:NamedIndividual rdf:about="http://purl.obolibrary.org/obo/GAZ_00237116">
        <obo:RO_0001025 rdf:resource="http://purl.obolibrary.org/obo/GAZ_00015519"/>
        <obo:IAO_0000115>A fourth-level administrative division of Uganda.</obo:IAO_0000115>
        <oboInOwl:hasOBONamespace>GAZ</oboInOwl:hasOBONamespace>
        <oboInOwl:id>GAZ:00237116</oboInOwl:id>
        <rdfs:label>Puranga Sub-county</rdfs:label>
    </owl:NamedIndividual>
    


    <!-- http://purl.obolibrary.org/obo/GAZ_00237117 -->

    <owl:NamedIndividual rdf:about="http://purl.obolibrary.org/obo/GAZ_00237117">
        <obo:IAO_0000115>A fourth-level administrative division of Uganda.</obo:IAO_0000115>
        <oboInOwl:hasOBONamespace>GAZ</oboInOwl:hasOBONamespace>
        <oboInOwl:id>GAZ:00237117</oboInOwl:id>
        <rdfs:label>Apo Sub-County</rdfs:label>
    </owl:NamedIndividual>
    


    <!-- http://purl.obolibrary.org/obo/GAZ_00237118 -->

    <owl:NamedIndividual rdf:about="http://purl.obolibrary.org/obo/GAZ_00237118">
        <obo:IAO_0000115>A fourth-level administrative division of Uganda.</obo:IAO_0000115>
        <oboInOwl:hasOBONamespace>GAZ</oboInOwl:hasOBONamespace>
        <oboInOwl:id>GAZ:00237118</oboInOwl:id>
        <rdfs:label>Drajani Sub-County</rdfs:label>
    </owl:NamedIndividual>
    


    <!-- http://purl.obolibrary.org/obo/GAZ_00237119 -->

    <owl:NamedIndividual rdf:about="http://purl.obolibrary.org/obo/GAZ_00237119">
        <obo:IAO_0000115>A fourth-level administrative division of Uganda.</obo:IAO_0000115>
        <oboInOwl:hasOBONamespace>GAZ</oboInOwl:hasOBONamespace>
        <oboInOwl:id>GAZ:00237119</oboInOwl:id>
        <rdfs:label>Kei Sub-County</rdfs:label>
    </owl:NamedIndividual>
    


    <!-- http://purl.obolibrary.org/obo/GAZ_00237120 -->

    <owl:NamedIndividual rdf:about="http://purl.obolibrary.org/obo/GAZ_00237120">
        <obo:IAO_0000115>A fourth-level administrative division of Uganda.</obo:IAO_0000115>
        <oboInOwl:hasOBONamespace>GAZ</oboInOwl:hasOBONamespace>
        <oboInOwl:id>GAZ:00237120</oboInOwl:id>
        <rdfs:label>Kuru Sub-County</rdfs:label>
    </owl:NamedIndividual>
    


    <!-- http://purl.obolibrary.org/obo/GAZ_00237121 -->

    <owl:NamedIndividual rdf:about="http://purl.obolibrary.org/obo/GAZ_00237121">
        <obo:IAO_0000115>A fourth-level administrative division of Uganda.</obo:IAO_0000115>
        <oboInOwl:hasOBONamespace>GAZ</oboInOwl:hasOBONamespace>
        <oboInOwl:id>GAZ:00237121</oboInOwl:id>
        <rdfs:label>Midigo Sub-County</rdfs:label>
    </owl:NamedIndividual>
    


    <!-- http://purl.obolibrary.org/obo/GAZ_00237122 -->

    <owl:NamedIndividual rdf:about="http://purl.obolibrary.org/obo/GAZ_00237122">
        <obo:IAO_0000115>A fourth-level administrative division of Uganda.</obo:IAO_0000115>
        <oboInOwl:hasOBONamespace>GAZ</oboInOwl:hasOBONamespace>
        <oboInOwl:id>GAZ:00237122</oboInOwl:id>
        <rdfs:label>Odravu Sub-County</rdfs:label>
    </owl:NamedIndividual>
    


    <!-- http://purl.obolibrary.org/obo/GAZ_00237123 -->

    <owl:NamedIndividual rdf:about="http://purl.obolibrary.org/obo/GAZ_00237123">
        <obo:IAO_0000115>A fourth-level administrative division of Uganda.</obo:IAO_0000115>
        <oboInOwl:hasOBONamespace>GAZ</oboInOwl:hasOBONamespace>
        <oboInOwl:id>GAZ:00237123</oboInOwl:id>
        <rdfs:label>Romogi Sub-County</rdfs:label>
    </owl:NamedIndividual>
    


    <!-- http://purl.obolibrary.org/obo/GAZ_00237124 -->

    <owl:NamedIndividual rdf:about="http://purl.obolibrary.org/obo/GAZ_00237124">
        <obo:IAO_0000115>A fourth-level administrative division of Uganda.</obo:IAO_0000115>
        <oboInOwl:hasOBONamespace>GAZ</oboInOwl:hasOBONamespace>
        <oboInOwl:id>GAZ:00237124</oboInOwl:id>
        <rdfs:label>Yumbe Town</rdfs:label>
    </owl:NamedIndividual>
    


    <!-- http://purl.obolibrary.org/obo/GAZ_00237125 -->

    <owl:NamedIndividual rdf:about="http://purl.obolibrary.org/obo/GAZ_00237125">
        <obo:IAO_0000115>A fourth-level administrative division of Uganda.</obo:IAO_0000115>
        <oboInOwl:hasOBONamespace>GAZ</oboInOwl:hasOBONamespace>
        <oboInOwl:id>GAZ:00237125</oboInOwl:id>
        <rdfs:label>Biiso Sub-county</rdfs:label>
    </owl:NamedIndividual>
    


    <!-- http://purl.obolibrary.org/obo/GAZ_00237126 -->

    <owl:NamedIndividual rdf:about="http://purl.obolibrary.org/obo/GAZ_00237126">
        <obo:IAO_0000115>A fourth-level administrative division of Uganda.</obo:IAO_0000115>
        <oboInOwl:hasOBONamespace>GAZ</oboInOwl:hasOBONamespace>
        <oboInOwl:id>GAZ:00237126</oboInOwl:id>
        <rdfs:label>Buliisa Sub-county</rdfs:label>
    </owl:NamedIndividual>
    


    <!-- http://purl.obolibrary.org/obo/GAZ_00237127 -->

    <owl:NamedIndividual rdf:about="http://purl.obolibrary.org/obo/GAZ_00237127">
        <obo:RO_0001025 rdf:resource="http://purl.obolibrary.org/obo/GAZ_00015558"/>
        <obo:IAO_0000115>A fourth-level administrative division of Uganda.</obo:IAO_0000115>
        <oboInOwl:hasOBONamespace>GAZ</oboInOwl:hasOBONamespace>
        <oboInOwl:id>GAZ:00237127</oboInOwl:id>
        <rdfs:label>Kasitu Sub-county</rdfs:label>
    </owl:NamedIndividual>
    


    <!-- http://purl.obolibrary.org/obo/GAZ_00237128 -->

    <owl:NamedIndividual rdf:about="http://purl.obolibrary.org/obo/GAZ_00237128">
        <obo:RO_0001025 rdf:resource="http://purl.obolibrary.org/obo/GAZ_00015558"/>
        <obo:IAO_0000115>A fourth-level administrative division of Uganda.</obo:IAO_0000115>
        <oboInOwl:hasOBONamespace>GAZ</oboInOwl:hasOBONamespace>
        <oboInOwl:id>GAZ:00237128</oboInOwl:id>
        <rdfs:label>Nduguto Sub-county</rdfs:label>
    </owl:NamedIndividual>
    


    <!-- http://purl.obolibrary.org/obo/GAZ_00237129 -->

    <owl:NamedIndividual rdf:about="http://purl.obolibrary.org/obo/GAZ_00237129">
        <obo:RO_0001025 rdf:resource="http://purl.obolibrary.org/obo/GAZ_00015558"/>
        <obo:IAO_0000115>A fourth-level administrative division of Uganda.</obo:IAO_0000115>
        <oboInOwl:hasOBONamespace>GAZ</oboInOwl:hasOBONamespace>
        <oboInOwl:id>GAZ:00237129</oboInOwl:id>
        <rdfs:label>Bubandi Sub-county</rdfs:label>
    </owl:NamedIndividual>
    


    <!-- http://purl.obolibrary.org/obo/GAZ_00237130 -->

    <owl:NamedIndividual rdf:about="http://purl.obolibrary.org/obo/GAZ_00237130">
        <obo:RO_0001025 rdf:resource="http://purl.obolibrary.org/obo/GAZ_00015558"/>
        <obo:IAO_0000115>A fourth-level administrative division of Uganda.</obo:IAO_0000115>
        <oboInOwl:hasOBONamespace>GAZ</oboInOwl:hasOBONamespace>
        <oboInOwl:id>GAZ:00237130</oboInOwl:id>
        <rdfs:label>Bubukwanga Sub-county</rdfs:label>
    </owl:NamedIndividual>
    


    <!-- http://purl.obolibrary.org/obo/GAZ_00237131 -->

    <owl:NamedIndividual rdf:about="http://purl.obolibrary.org/obo/GAZ_00237131">
        <obo:RO_0001025 rdf:resource="http://purl.obolibrary.org/obo/GAZ_00015558"/>
        <obo:IAO_0000115>A fourth-level administrative division of Uganda.</obo:IAO_0000115>
        <oboInOwl:hasOBONamespace>GAZ</oboInOwl:hasOBONamespace>
        <oboInOwl:id>GAZ:00237131</oboInOwl:id>
        <rdfs:label>Bundibugyo Town</rdfs:label>
    </owl:NamedIndividual>
    


    <!-- http://purl.obolibrary.org/obo/GAZ_00237132 -->

    <owl:NamedIndividual rdf:about="http://purl.obolibrary.org/obo/GAZ_00237132">
        <obo:RO_0001025 rdf:resource="http://purl.obolibrary.org/obo/GAZ_00015558"/>
        <obo:IAO_0000115>A fourth-level administrative division of Uganda.</obo:IAO_0000115>
        <oboInOwl:hasOBONamespace>GAZ</oboInOwl:hasOBONamespace>
        <oboInOwl:id>GAZ:00237132</oboInOwl:id>
        <rdfs:label>Busaru Sub-county</rdfs:label>
    </owl:NamedIndividual>
    


    <!-- http://purl.obolibrary.org/obo/GAZ_00237133 -->

    <owl:NamedIndividual rdf:about="http://purl.obolibrary.org/obo/GAZ_00237133">
        <obo:RO_0001025 rdf:resource="http://purl.obolibrary.org/obo/GAZ_00015558"/>
        <obo:IAO_0000115>A fourth-level administrative division of Uganda.</obo:IAO_0000115>
        <oboInOwl:hasOBONamespace>GAZ</oboInOwl:hasOBONamespace>
        <oboInOwl:id>GAZ:00237133</oboInOwl:id>
        <rdfs:label>Harugali Sub-county</rdfs:label>
    </owl:NamedIndividual>
    


    <!-- http://purl.obolibrary.org/obo/GAZ_00237134 -->

    <owl:NamedIndividual rdf:about="http://purl.obolibrary.org/obo/GAZ_00237134">
        <obo:RO_0001025 rdf:resource="http://purl.obolibrary.org/obo/GAZ_00015559"/>
        <obo:IAO_0000115>A fourth-level administrative division of Uganda.</obo:IAO_0000115>
        <oboInOwl:hasOBONamespace>GAZ</oboInOwl:hasOBONamespace>
        <oboInOwl:id>GAZ:00237134</oboInOwl:id>
        <rdfs:label>Kanara Sub-county</rdfs:label>
    </owl:NamedIndividual>
    


    <!-- http://purl.obolibrary.org/obo/GAZ_00237135 -->

    <owl:NamedIndividual rdf:about="http://purl.obolibrary.org/obo/GAZ_00237135">
        <obo:RO_0001025 rdf:resource="http://purl.obolibrary.org/obo/GAZ_00015559"/>
        <obo:IAO_0000115>A fourth-level administrative division of Uganda.</obo:IAO_0000115>
        <oboInOwl:hasOBONamespace>GAZ</oboInOwl:hasOBONamespace>
        <oboInOwl:id>GAZ:00237135</oboInOwl:id>
        <rdfs:label>Karugutu Sub-county</rdfs:label>
    </owl:NamedIndividual>
    


    <!-- http://purl.obolibrary.org/obo/GAZ_00237136 -->

    <owl:NamedIndividual rdf:about="http://purl.obolibrary.org/obo/GAZ_00237136">
        <obo:RO_0001025 rdf:resource="http://purl.obolibrary.org/obo/GAZ_00015559"/>
        <obo:IAO_0000115>A fourth-level administrative division of Uganda.</obo:IAO_0000115>
        <oboInOwl:hasOBONamespace>GAZ</oboInOwl:hasOBONamespace>
        <oboInOwl:id>GAZ:00237136</oboInOwl:id>
        <rdfs:label>Rwebisengo Sub-county</rdfs:label>
    </owl:NamedIndividual>
    


    <!-- http://purl.obolibrary.org/obo/GAZ_00237137 -->

    <owl:NamedIndividual rdf:about="http://purl.obolibrary.org/obo/GAZ_00237137">
        <obo:RO_0001025 rdf:resource="http://purl.obolibrary.org/obo/GAZ_00076731"/>
        <obo:IAO_0000115>A wide, 32 km long body of water that links Lake Edward and Lake George, and a dominant feature of Queen Elizabeth National Park.</obo:IAO_0000115>
        <oboInOwl:hasOBONamespace>GAZ</oboInOwl:hasOBONamespace>
        <oboInOwl:id>GAZ:00237137</oboInOwl:id>
        <rdfs:label>Kazinga Channel</rdfs:label>
    </owl:NamedIndividual>
    


    <!-- http://purl.obolibrary.org/obo/GAZ_00237138 -->

    <owl:NamedIndividual rdf:about="http://purl.obolibrary.org/obo/GAZ_00237138">
        <obo:RO_0001025 rdf:resource="http://purl.obolibrary.org/obo/GAZ_00015553"/>
        <obo:IAO_0000115>A fourth-level administrative division of Uganda.</obo:IAO_0000115>
        <oboInOwl:hasOBONamespace>GAZ</oboInOwl:hasOBONamespace>
        <oboInOwl:id>GAZ:00237138</oboInOwl:id>
        <rdfs:label>Bihanga Sub-county</rdfs:label>
    </owl:NamedIndividual>
    


    <!-- http://purl.obolibrary.org/obo/GAZ_00237139 -->

    <owl:NamedIndividual rdf:about="http://purl.obolibrary.org/obo/GAZ_00237139">
        <obo:RO_0001025 rdf:resource="http://purl.obolibrary.org/obo/GAZ_00015553"/>
        <obo:IAO_0000115>A fourth-level administrative division of Uganda.</obo:IAO_0000115>
        <oboInOwl:hasOBONamespace>GAZ</oboInOwl:hasOBONamespace>
        <oboInOwl:id>GAZ:00237139</oboInOwl:id>
        <rdfs:label>Burere Sub-county</rdfs:label>
    </owl:NamedIndividual>
    


    <!-- http://purl.obolibrary.org/obo/GAZ_00237140 -->

    <owl:NamedIndividual rdf:about="http://purl.obolibrary.org/obo/GAZ_00237140">
        <obo:RO_0001025 rdf:resource="http://purl.obolibrary.org/obo/GAZ_00015553"/>
        <obo:IAO_0000115>A fourth-level administrative division of Uganda.</obo:IAO_0000115>
        <oboInOwl:hasOBONamespace>GAZ</oboInOwl:hasOBONamespace>
        <oboInOwl:id>GAZ:00237140</oboInOwl:id>
        <rdfs:label>Karungu Sub-county</rdfs:label>
    </owl:NamedIndividual>
    


    <!-- http://purl.obolibrary.org/obo/GAZ_00237141 -->

    <owl:NamedIndividual rdf:about="http://purl.obolibrary.org/obo/GAZ_00237141">
        <obo:RO_0001025 rdf:resource="http://purl.obolibrary.org/obo/GAZ_00015553"/>
        <obo:IAO_0000115>A fourth-level administrative division of Uganda.</obo:IAO_0000115>
        <oboInOwl:hasOBONamespace>GAZ</oboInOwl:hasOBONamespace>
        <oboInOwl:id>GAZ:00237141</oboInOwl:id>
        <rdfs:label>Rwengwe Sub-county</rdfs:label>
    </owl:NamedIndividual>
    


    <!-- http://purl.obolibrary.org/obo/GAZ_00237142 -->

    <owl:NamedIndividual rdf:about="http://purl.obolibrary.org/obo/GAZ_00237142">
        <obo:RO_0001025 rdf:resource="http://purl.obolibrary.org/obo/GAZ_00015556"/>
        <obo:IAO_0000115>A fourth-level administrative division of Uganda.</obo:IAO_0000115>
        <oboInOwl:hasOBONamespace>GAZ</oboInOwl:hasOBONamespace>
        <oboInOwl:id>GAZ:00237142</oboInOwl:id>
        <rdfs:label>Katerera Sub-county</rdfs:label>
    </owl:NamedIndividual>
    


    <!-- http://purl.obolibrary.org/obo/GAZ_00237143 -->

    <owl:NamedIndividual rdf:about="http://purl.obolibrary.org/obo/GAZ_00237143">
        <obo:RO_0001025 rdf:resource="http://purl.obolibrary.org/obo/GAZ_00015556"/>
        <obo:IAO_0000115>A fourth-level administrative division of Uganda.</obo:IAO_0000115>
        <oboInOwl:hasOBONamespace>GAZ</oboInOwl:hasOBONamespace>
        <oboInOwl:id>GAZ:00237143</oboInOwl:id>
        <rdfs:label>Katunguru Sub-county</rdfs:label>
    </owl:NamedIndividual>
    


    <!-- http://purl.obolibrary.org/obo/GAZ_00237144 -->

    <owl:NamedIndividual rdf:about="http://purl.obolibrary.org/obo/GAZ_00237144">
        <obo:RO_0001025 rdf:resource="http://purl.obolibrary.org/obo/GAZ_00015556"/>
        <obo:IAO_0000115>A fourth-level administrative division of Uganda.</obo:IAO_0000115>
        <oboInOwl:hasOBONamespace>GAZ</oboInOwl:hasOBONamespace>
        <oboInOwl:id>GAZ:00237144</oboInOwl:id>
        <rdfs:label>Kichwamba Sub-county</rdfs:label>
    </owl:NamedIndividual>
    


    <!-- http://purl.obolibrary.org/obo/GAZ_00237145 -->

    <owl:NamedIndividual rdf:about="http://purl.obolibrary.org/obo/GAZ_00237145">
        <obo:RO_0001025 rdf:resource="http://purl.obolibrary.org/obo/GAZ_00015556"/>
        <obo:IAO_0000115>A fourth-level administrative division of Uganda.</obo:IAO_0000115>
        <oboInOwl:hasOBONamespace>GAZ</oboInOwl:hasOBONamespace>
        <oboInOwl:id>GAZ:00237145</oboInOwl:id>
        <rdfs:label>Ryeru Sub-county</rdfs:label>
    </owl:NamedIndividual>
    


    <!-- http://purl.obolibrary.org/obo/GAZ_00237146 -->

    <owl:NamedIndividual rdf:about="http://purl.obolibrary.org/obo/GAZ_00237146">
        <obo:RO_0001025 rdf:resource="http://purl.obolibrary.org/obo/GAZ_00015554"/>
        <obo:IAO_0000115>A fourth-level administrative division of Uganda.</obo:IAO_0000115>
        <oboInOwl:hasOBONamespace>GAZ</oboInOwl:hasOBONamespace>
        <oboInOwl:id>GAZ:00237146</oboInOwl:id>
        <rdfs:label>Bumbaire Sub-county</rdfs:label>
    </owl:NamedIndividual>
    


    <!-- http://purl.obolibrary.org/obo/GAZ_00237147 -->

    <owl:NamedIndividual rdf:about="http://purl.obolibrary.org/obo/GAZ_00237147">
        <obo:RO_0001025 rdf:resource="http://purl.obolibrary.org/obo/GAZ_00015554"/>
        <obo:IAO_0000115>A fourth-level administrative division of Uganda.</obo:IAO_0000115>
        <oboInOwl:hasOBONamespace>GAZ</oboInOwl:hasOBONamespace>
        <oboInOwl:id>GAZ:00237147</oboInOwl:id>
        <rdfs:label>Bushenyi Town</rdfs:label>
    </owl:NamedIndividual>
    


    <!-- http://purl.obolibrary.org/obo/GAZ_00237148 -->

    <owl:NamedIndividual rdf:about="http://purl.obolibrary.org/obo/GAZ_00237148">
        <obo:RO_0001025 rdf:resource="http://purl.obolibrary.org/obo/GAZ_00015554"/>
        <obo:IAO_0000115>A fourth-level administrative division of Uganda.</obo:IAO_0000115>
        <oboInOwl:hasOBONamespace>GAZ</oboInOwl:hasOBONamespace>
        <oboInOwl:id>GAZ:00237148</oboInOwl:id>
        <rdfs:label>Kakanju Sub-county</rdfs:label>
    </owl:NamedIndividual>
    


    <!-- http://purl.obolibrary.org/obo/GAZ_00237149 -->

    <owl:NamedIndividual rdf:about="http://purl.obolibrary.org/obo/GAZ_00237149">
        <obo:RO_0001025 rdf:resource="http://purl.obolibrary.org/obo/GAZ_00015554"/>
        <obo:IAO_0000115>A fourth-level administrative division of Uganda.</obo:IAO_0000115>
        <oboInOwl:hasOBONamespace>GAZ</oboInOwl:hasOBONamespace>
        <oboInOwl:id>GAZ:00237149</oboInOwl:id>
        <rdfs:label>Kyabugimbi Sub-county</rdfs:label>
    </owl:NamedIndividual>
    


    <!-- http://purl.obolibrary.org/obo/GAZ_00237150 -->

    <owl:NamedIndividual rdf:about="http://purl.obolibrary.org/obo/GAZ_00237150">
        <obo:RO_0001025 rdf:resource="http://purl.obolibrary.org/obo/GAZ_00015554"/>
        <obo:IAO_0000115>A fourth-level administrative division of Uganda.</obo:IAO_0000115>
        <oboInOwl:hasOBONamespace>GAZ</oboInOwl:hasOBONamespace>
        <oboInOwl:id>GAZ:00237150</oboInOwl:id>
        <rdfs:label>Kyamuhunga Sub-county</rdfs:label>
    </owl:NamedIndividual>
    


    <!-- http://purl.obolibrary.org/obo/GAZ_00237151 -->

    <owl:NamedIndividual rdf:about="http://purl.obolibrary.org/obo/GAZ_00237151">
        <obo:RO_0001025 rdf:resource="http://purl.obolibrary.org/obo/GAZ_00015554"/>
        <obo:IAO_0000115>A fourth-level administrative division of Uganda.</obo:IAO_0000115>
        <oboInOwl:hasOBONamespace>GAZ</oboInOwl:hasOBONamespace>
        <oboInOwl:id>GAZ:00237151</oboInOwl:id>
        <rdfs:label>Kyeizoba Sub-county</rdfs:label>
    </owl:NamedIndividual>
    


    <!-- http://purl.obolibrary.org/obo/GAZ_00237152 -->

    <owl:NamedIndividual rdf:about="http://purl.obolibrary.org/obo/GAZ_00237152">
        <obo:RO_0001025 rdf:resource="http://purl.obolibrary.org/obo/GAZ_00015554"/>
        <obo:IAO_0000115>A fourth-level administrative division of Uganda.</obo:IAO_0000115>
        <oboInOwl:hasOBONamespace>GAZ</oboInOwl:hasOBONamespace>
        <oboInOwl:id>GAZ:00237152</oboInOwl:id>
        <rdfs:label>Nyabubare Sub-county</rdfs:label>
    </owl:NamedIndividual>
    


    <!-- http://purl.obolibrary.org/obo/GAZ_00237153 -->

    <owl:NamedIndividual rdf:about="http://purl.obolibrary.org/obo/GAZ_00237153">
        <obo:RO_0001025 rdf:resource="http://purl.obolibrary.org/obo/GAZ_00015557"/>
        <obo:IAO_0000115>A fourth-level administrative division of Uganda.</obo:IAO_0000115>
        <oboInOwl:hasOBONamespace>GAZ</oboInOwl:hasOBONamespace>
        <oboInOwl:id>GAZ:00237153</oboInOwl:id>
        <rdfs:label>Bitereko Sub-county</rdfs:label>
    </owl:NamedIndividual>
    


    <!-- http://purl.obolibrary.org/obo/GAZ_00237154 -->

    <owl:NamedIndividual rdf:about="http://purl.obolibrary.org/obo/GAZ_00237154">
        <obo:RO_0001025 rdf:resource="http://purl.obolibrary.org/obo/GAZ_00015557"/>
        <obo:IAO_0000115>A fourth-level administrative division of Uganda.</obo:IAO_0000115>
        <oboInOwl:hasOBONamespace>GAZ</oboInOwl:hasOBONamespace>
        <oboInOwl:id>GAZ:00237154</oboInOwl:id>
        <rdfs:label>Kabira Sub-county</rdfs:label>
    </owl:NamedIndividual>
    


    <!-- http://purl.obolibrary.org/obo/GAZ_00237155 -->

    <owl:NamedIndividual rdf:about="http://purl.obolibrary.org/obo/GAZ_00237155">
        <obo:RO_0001025 rdf:resource="http://purl.obolibrary.org/obo/GAZ_00015557"/>
        <obo:IAO_0000115>A fourth-level administrative division of Uganda.</obo:IAO_0000115>
        <oboInOwl:hasOBONamespace>GAZ</oboInOwl:hasOBONamespace>
        <oboInOwl:id>GAZ:00237155</oboInOwl:id>
        <rdfs:label>Kanyabwanga Sub-county</rdfs:label>
    </owl:NamedIndividual>
    


    <!-- http://purl.obolibrary.org/obo/GAZ_00237156 -->

    <owl:NamedIndividual rdf:about="http://purl.obolibrary.org/obo/GAZ_00237156">
        <obo:RO_0001025 rdf:resource="http://purl.obolibrary.org/obo/GAZ_00015557"/>
        <obo:IAO_0000115>A fourth-level administrative division of Uganda.</obo:IAO_0000115>
        <oboInOwl:hasOBONamespace>GAZ</oboInOwl:hasOBONamespace>
        <oboInOwl:id>GAZ:00237156</oboInOwl:id>
        <rdfs:label>Kashenshero Sub-county</rdfs:label>
    </owl:NamedIndividual>
    


    <!-- http://purl.obolibrary.org/obo/GAZ_00237157 -->

    <owl:NamedIndividual rdf:about="http://purl.obolibrary.org/obo/GAZ_00237157">
        <obo:RO_0001025 rdf:resource="http://purl.obolibrary.org/obo/GAZ_00015557"/>
        <obo:IAO_0000115>A fourth-level administrative division of Uganda.</obo:IAO_0000115>
        <oboInOwl:hasOBONamespace>GAZ</oboInOwl:hasOBONamespace>
        <oboInOwl:id>GAZ:00237157</oboInOwl:id>
        <rdfs:label>Kiyanga Sub-county</rdfs:label>
    </owl:NamedIndividual>
    


    <!-- http://purl.obolibrary.org/obo/GAZ_00237158 -->

    <owl:NamedIndividual rdf:about="http://purl.obolibrary.org/obo/GAZ_00237158">
        <obo:RO_0001025 rdf:resource="http://purl.obolibrary.org/obo/GAZ_00015557"/>
        <obo:IAO_0000115>A fourth-level administrative division of Uganda.</obo:IAO_0000115>
        <oboInOwl:hasOBONamespace>GAZ</oboInOwl:hasOBONamespace>
        <oboInOwl:id>GAZ:00237158</oboInOwl:id>
        <rdfs:label>Mitooma Sub-county</rdfs:label>
    </owl:NamedIndividual>
    


    <!-- http://purl.obolibrary.org/obo/GAZ_00237159 -->

    <owl:NamedIndividual rdf:about="http://purl.obolibrary.org/obo/GAZ_00237159">
        <obo:RO_0001025 rdf:resource="http://purl.obolibrary.org/obo/GAZ_00015557"/>
        <obo:IAO_0000115>A fourth-level administrative division of Uganda.</obo:IAO_0000115>
        <oboInOwl:hasOBONamespace>GAZ</oboInOwl:hasOBONamespace>
        <oboInOwl:id>GAZ:00237159</oboInOwl:id>
        <rdfs:label>Mutara Sub-county</rdfs:label>
    </owl:NamedIndividual>
    


    <!-- http://purl.obolibrary.org/obo/GAZ_00237160 -->

    <owl:NamedIndividual rdf:about="http://purl.obolibrary.org/obo/GAZ_00237160">
        <obo:RO_0001025 rdf:resource="http://purl.obolibrary.org/obo/GAZ_00015555"/>
        <obo:IAO_0000115>A fourth-level administrative division of Uganda.</obo:IAO_0000115>
        <oboInOwl:hasOBONamespace>GAZ</oboInOwl:hasOBONamespace>
        <oboInOwl:id>GAZ:00237160</oboInOwl:id>
        <rdfs:label>Bugongi Sub-county</rdfs:label>
    </owl:NamedIndividual>
    


    <!-- http://purl.obolibrary.org/obo/GAZ_00237161 -->

    <owl:NamedIndividual rdf:about="http://purl.obolibrary.org/obo/GAZ_00237161">
        <obo:RO_0001025 rdf:resource="http://purl.obolibrary.org/obo/GAZ_00015555"/>
        <obo:IAO_0000115>A fourth-level administrative division of Uganda.</obo:IAO_0000115>
        <oboInOwl:hasOBONamespace>GAZ</oboInOwl:hasOBONamespace>
        <oboInOwl:id>GAZ:00237161</oboInOwl:id>
        <rdfs:label>Kabwohe-Itendero Town</rdfs:label>
    </owl:NamedIndividual>
    


    <!-- http://purl.obolibrary.org/obo/GAZ_00237162 -->

    <owl:NamedIndividual rdf:about="http://purl.obolibrary.org/obo/GAZ_00237162">
        <obo:RO_0001025 rdf:resource="http://purl.obolibrary.org/obo/GAZ_00015555"/>
        <obo:IAO_0000115>A fourth-level administrative division of Uganda.</obo:IAO_0000115>
        <oboInOwl:hasOBONamespace>GAZ</oboInOwl:hasOBONamespace>
        <oboInOwl:id>GAZ:00237162</oboInOwl:id>
        <rdfs:label>Kagango Sub-county</rdfs:label>
    </owl:NamedIndividual>
    


    <!-- http://purl.obolibrary.org/obo/GAZ_00237163 -->

    <owl:NamedIndividual rdf:about="http://purl.obolibrary.org/obo/GAZ_00237163">
        <obo:RO_0001025 rdf:resource="http://purl.obolibrary.org/obo/GAZ_00015555"/>
        <obo:IAO_0000115>A fourth-level administrative division of Uganda.</obo:IAO_0000115>
        <oboInOwl:hasOBONamespace>GAZ</oboInOwl:hasOBONamespace>
        <oboInOwl:id>GAZ:00237163</oboInOwl:id>
        <rdfs:label>Kigarama Sub-county</rdfs:label>
    </owl:NamedIndividual>
    


    <!-- http://purl.obolibrary.org/obo/GAZ_00237164 -->

    <owl:NamedIndividual rdf:about="http://purl.obolibrary.org/obo/GAZ_00237164">
        <obo:RO_0001025 rdf:resource="http://purl.obolibrary.org/obo/GAZ_00015555"/>
        <obo:IAO_0000115>A fourth-level administrative division of Uganda.</obo:IAO_0000115>
        <oboInOwl:hasOBONamespace>GAZ</oboInOwl:hasOBONamespace>
        <oboInOwl:id>GAZ:00237164</oboInOwl:id>
        <rdfs:label>Kitagata Sub-county</rdfs:label>
    </owl:NamedIndividual>
    


    <!-- http://purl.obolibrary.org/obo/GAZ_00237165 -->

    <owl:NamedIndividual rdf:about="http://purl.obolibrary.org/obo/GAZ_00237165">
        <obo:RO_0001025 rdf:resource="http://purl.obolibrary.org/obo/GAZ_00015555"/>
        <obo:IAO_0000115>A fourth-level administrative division of Uganda.</obo:IAO_0000115>
        <oboInOwl:hasOBONamespace>GAZ</oboInOwl:hasOBONamespace>
        <oboInOwl:id>GAZ:00237165</oboInOwl:id>
        <rdfs:label>Kyangyenyi Sub-county</rdfs:label>
    </owl:NamedIndividual>
    


    <!-- http://purl.obolibrary.org/obo/GAZ_00237166 -->

    <owl:NamedIndividual rdf:about="http://purl.obolibrary.org/obo/GAZ_00237166">
        <obo:RO_0001025 rdf:resource="http://purl.obolibrary.org/obo/GAZ_00015555"/>
        <obo:IAO_0000115>A fourth-level administrative division of Uganda.</obo:IAO_0000115>
        <oboInOwl:hasOBONamespace>GAZ</oboInOwl:hasOBONamespace>
        <oboInOwl:id>GAZ:00237166</oboInOwl:id>
        <rdfs:label>Shuuku Sub-county</rdfs:label>
    </owl:NamedIndividual>
    


    <!-- http://purl.obolibrary.org/obo/GAZ_00237167 -->

    <owl:NamedIndividual rdf:about="http://purl.obolibrary.org/obo/GAZ_00237167">
        <obo:RO_0001025 rdf:resource="http://purl.obolibrary.org/obo/GAZ_00076731"/>
        <obo:IAO_0000115>A protected area. A part of the Queen Elizabeth National Park (QENP) in Uganda.</obo:IAO_0000115>
        <oboInOwl:hasOBONamespace>GAZ</oboInOwl:hasOBONamespace>
        <oboInOwl:id>GAZ:00237167</oboInOwl:id>
        <rdfs:label>Kyambura Game Reserve</rdfs:label>
    </owl:NamedIndividual>
    


    <!-- http://purl.obolibrary.org/obo/GAZ_00237174 -->

    <owl:NamedIndividual rdf:about="http://purl.obolibrary.org/obo/GAZ_00237174">
        <obo:IAO_0000115>A hydroelectric power station across the White Nile near to its source at Lake Victoria in Uganda.</obo:IAO_0000115>
        <oboInOwl:hasOBONamespace>GAZ</oboInOwl:hasOBONamespace>
        <oboInOwl:id>GAZ:00237174</oboInOwl:id>
        <rdfs:label>Nalubaale Power Station</rdfs:label>
    </owl:NamedIndividual>
    


    <!-- http://purl.obolibrary.org/obo/GAZ_00237175 -->

    <owl:NamedIndividual rdf:about="http://purl.obolibrary.org/obo/GAZ_00237175">
        <obo:RO_0001025 rdf:resource="http://purl.obolibrary.org/obo/GAZ_00015466"/>
        <obo:IAO_0000115>A hydroelectric power station located in Jinja, Jinja District, in eastern central Uganda.</obo:IAO_0000115>
        <oboInOwl:hasOBONamespace>GAZ</oboInOwl:hasOBONamespace>
        <oboInOwl:id>GAZ:00237175</oboInOwl:id>
        <rdfs:label>Kiira Power Station</rdfs:label>
    </owl:NamedIndividual>
    


    <!-- http://purl.obolibrary.org/obo/GAZ_00237176 -->

    <owl:NamedIndividual rdf:about="http://purl.obolibrary.org/obo/GAZ_00237176">
        <obo:RO_0001025 rdf:resource="http://purl.obolibrary.org/obo/GAZ_00015351"/>
        <obo:IAO_0000115>A hydroelectric power project located at the headwaters of River Nile, about 16 km north of Jinja at the former location of Bujagali Falls.</obo:IAO_0000115>
        <oboInOwl:hasOBONamespace>GAZ</oboInOwl:hasOBONamespace>
        <oboInOwl:id>GAZ:00237176</oboInOwl:id>
        <rdfs:label>Bujagali Power Station</rdfs:label>
    </owl:NamedIndividual>
    


    <!-- http://purl.obolibrary.org/obo/GAZ_00237177 -->

    <owl:NamedIndividual rdf:about="http://purl.obolibrary.org/obo/GAZ_00237177">
        <obo:RO_0001025 rdf:resource="http://purl.obolibrary.org/obo/GAZ_00015551"/>
        <obo:IAO_0000115>A fourth-level administrative division of Uganda.</obo:IAO_0000115>
        <oboInOwl:hasOBONamespace>GAZ</oboInOwl:hasOBONamespace>
        <oboInOwl:id>GAZ:00237177</oboInOwl:id>
        <rdfs:label>Buhanika Sub-county</rdfs:label>
    </owl:NamedIndividual>
    


    <!-- http://purl.obolibrary.org/obo/GAZ_00237178 -->

    <owl:NamedIndividual rdf:about="http://purl.obolibrary.org/obo/GAZ_00237178">
        <obo:RO_0001025 rdf:resource="http://purl.obolibrary.org/obo/GAZ_00015551"/>
        <obo:IAO_0000115>A fourth-level administrative division of Uganda.</obo:IAO_0000115>
        <oboInOwl:hasOBONamespace>GAZ</oboInOwl:hasOBONamespace>
        <oboInOwl:id>GAZ:00237178</oboInOwl:id>
        <rdfs:label>Buseruka Sub-county</rdfs:label>
    </owl:NamedIndividual>
    


    <!-- http://purl.obolibrary.org/obo/GAZ_00237179 -->

    <owl:NamedIndividual rdf:about="http://purl.obolibrary.org/obo/GAZ_00237179">
        <obo:RO_0001025 rdf:resource="http://purl.obolibrary.org/obo/GAZ_00015551"/>
        <obo:IAO_0000115>A fourth-level administrative division of Uganda.</obo:IAO_0000115>
        <oboInOwl:hasOBONamespace>GAZ</oboInOwl:hasOBONamespace>
        <oboInOwl:id>GAZ:00237179</oboInOwl:id>
        <rdfs:label>Busiisi Sub-county</rdfs:label>
    </owl:NamedIndividual>
    


    <!-- http://purl.obolibrary.org/obo/GAZ_00237180 -->

    <owl:NamedIndividual rdf:about="http://purl.obolibrary.org/obo/GAZ_00237180">
        <obo:RO_0001025 rdf:resource="http://purl.obolibrary.org/obo/GAZ_00015551"/>
        <obo:IAO_0000115>A fourth-level administrative division of Uganda.</obo:IAO_0000115>
        <oboInOwl:hasOBONamespace>GAZ</oboInOwl:hasOBONamespace>
        <oboInOwl:id>GAZ:00237180</oboInOwl:id>
        <rdfs:label>Hoima Town</rdfs:label>
    </owl:NamedIndividual>
    


    <!-- http://purl.obolibrary.org/obo/GAZ_00237181 -->

    <owl:NamedIndividual rdf:about="http://purl.obolibrary.org/obo/GAZ_00237181">
        <obo:RO_0001025 rdf:resource="http://purl.obolibrary.org/obo/GAZ_00015551"/>
        <obo:IAO_0000115>A fourth-level administrative division of Uganda.</obo:IAO_0000115>
        <oboInOwl:hasOBONamespace>GAZ</oboInOwl:hasOBONamespace>
        <oboInOwl:id>GAZ:00237181</oboInOwl:id>
        <rdfs:label>Kigorobya Town</rdfs:label>
    </owl:NamedIndividual>
    


    <!-- http://purl.obolibrary.org/obo/GAZ_00237182 -->

    <owl:NamedIndividual rdf:about="http://purl.obolibrary.org/obo/GAZ_00237182">
        <obo:RO_0001025 rdf:resource="http://purl.obolibrary.org/obo/GAZ_00015551"/>
        <obo:IAO_0000115>A fourth-level administrative division of Uganda.</obo:IAO_0000115>
        <oboInOwl:hasOBONamespace>GAZ</oboInOwl:hasOBONamespace>
        <oboInOwl:id>GAZ:00237182</oboInOwl:id>
        <rdfs:label>Kigorobya Sub-county</rdfs:label>
    </owl:NamedIndividual>
    


    <!-- http://purl.obolibrary.org/obo/GAZ_00237183 -->

    <owl:NamedIndividual rdf:about="http://purl.obolibrary.org/obo/GAZ_00237183">
        <obo:RO_0001025 rdf:resource="http://purl.obolibrary.org/obo/GAZ_00015551"/>
        <obo:IAO_0000115>A fourth-level administrative division of Uganda.</obo:IAO_0000115>
        <oboInOwl:hasOBONamespace>GAZ</oboInOwl:hasOBONamespace>
        <oboInOwl:id>GAZ:00237183</oboInOwl:id>
        <rdfs:label>Kitoba Sub-county</rdfs:label>
    </owl:NamedIndividual>
    


    <!-- http://purl.obolibrary.org/obo/GAZ_00237184 -->

    <owl:NamedIndividual rdf:about="http://purl.obolibrary.org/obo/GAZ_00237184">
        <obo:RO_0001025 rdf:resource="http://purl.obolibrary.org/obo/GAZ_00015551"/>
        <obo:IAO_0000115>A fourth-level administrative division of Uganda.</obo:IAO_0000115>
        <oboInOwl:hasOBONamespace>GAZ</oboInOwl:hasOBONamespace>
        <oboInOwl:id>GAZ:00237184</oboInOwl:id>
        <rdfs:label>Kyabigambire Sub-county</rdfs:label>
    </owl:NamedIndividual>
    


    <!-- http://purl.obolibrary.org/obo/GAZ_00237185 -->

    <owl:NamedIndividual rdf:about="http://purl.obolibrary.org/obo/GAZ_00237185">
        <obo:RO_0001025 rdf:resource="http://purl.obolibrary.org/obo/GAZ_00015552"/>
        <obo:IAO_0000115>A fourth-level administrative division of Uganda.</obo:IAO_0000115>
        <oboInOwl:hasOBONamespace>GAZ</oboInOwl:hasOBONamespace>
        <oboInOwl:id>GAZ:00237185</oboInOwl:id>
        <rdfs:label>Bugambe Sub-county</rdfs:label>
    </owl:NamedIndividual>
    


    <!-- http://purl.obolibrary.org/obo/GAZ_00237186 -->

    <owl:NamedIndividual rdf:about="http://purl.obolibrary.org/obo/GAZ_00237186">
        <obo:RO_0001025 rdf:resource="http://purl.obolibrary.org/obo/GAZ_00015552"/>
        <obo:IAO_0000115>A fourth-level administrative division of Uganda.</obo:IAO_0000115>
        <oboInOwl:hasOBONamespace>GAZ</oboInOwl:hasOBONamespace>
        <oboInOwl:id>GAZ:00237186</oboInOwl:id>
        <rdfs:label>Buhimba Sub-county</rdfs:label>
    </owl:NamedIndividual>
    


    <!-- http://purl.obolibrary.org/obo/GAZ_00237187 -->

    <owl:NamedIndividual rdf:about="http://purl.obolibrary.org/obo/GAZ_00237187">
        <obo:RO_0001025 rdf:resource="http://purl.obolibrary.org/obo/GAZ_00015552"/>
        <obo:IAO_0000115>A fourth-level administrative division of Uganda.</obo:IAO_0000115>
        <oboInOwl:hasOBONamespace>GAZ</oboInOwl:hasOBONamespace>
        <oboInOwl:id>GAZ:00237187</oboInOwl:id>
        <rdfs:label>Kabwoya Sub-county</rdfs:label>
    </owl:NamedIndividual>
    


    <!-- http://purl.obolibrary.org/obo/GAZ_00237188 -->

    <owl:NamedIndividual rdf:about="http://purl.obolibrary.org/obo/GAZ_00237188">
        <obo:RO_0001025 rdf:resource="http://purl.obolibrary.org/obo/GAZ_00015552"/>
        <obo:IAO_0000115>A fourth-level administrative division of Uganda.</obo:IAO_0000115>
        <oboInOwl:hasOBONamespace>GAZ</oboInOwl:hasOBONamespace>
        <oboInOwl:id>GAZ:00237188</oboInOwl:id>
        <rdfs:label>Kiziranfumbi Sub-county</rdfs:label>
    </owl:NamedIndividual>
    


    <!-- http://purl.obolibrary.org/obo/GAZ_00237189 -->

    <owl:NamedIndividual rdf:about="http://purl.obolibrary.org/obo/GAZ_00237189">
        <obo:RO_0001025 rdf:resource="http://purl.obolibrary.org/obo/GAZ_00015552"/>
        <obo:IAO_0000115>A fourth-level administrative division of Uganda.</obo:IAO_0000115>
        <oboInOwl:hasOBONamespace>GAZ</oboInOwl:hasOBONamespace>
        <oboInOwl:id>GAZ:00237189</oboInOwl:id>
        <rdfs:label>Kyangwali Sub-county</rdfs:label>
    </owl:NamedIndividual>
    


    <!-- http://purl.obolibrary.org/obo/GAZ_00237190 -->

    <owl:NamedIndividual rdf:about="http://purl.obolibrary.org/obo/GAZ_00237190">
        <obo:IAO_0000115>A fourth-level administrative division of Uganda.</obo:IAO_0000115>
        <oboInOwl:hasOBONamespace>GAZ</oboInOwl:hasOBONamespace>
        <oboInOwl:id>GAZ:00237190</oboInOwl:id>
        <rdfs:label>Bisheshe Sub-county</rdfs:label>
    </owl:NamedIndividual>
    


    <!-- http://purl.obolibrary.org/obo/GAZ_00237191 -->

    <owl:NamedIndividual rdf:about="http://purl.obolibrary.org/obo/GAZ_00237191">
        <obo:IAO_0000115>A fourth-level administrative division of Uganda.</obo:IAO_0000115>
        <oboInOwl:hasOBONamespace>GAZ</oboInOwl:hasOBONamespace>
        <oboInOwl:id>GAZ:00237191</oboInOwl:id>
        <rdfs:label>Ibanda Town</rdfs:label>
    </owl:NamedIndividual>
    


    <!-- http://purl.obolibrary.org/obo/GAZ_00237192 -->

    <owl:NamedIndividual rdf:about="http://purl.obolibrary.org/obo/GAZ_00237192">
        <obo:IAO_0000115>A fourth-level administrative division of Uganda.</obo:IAO_0000115>
        <oboInOwl:hasOBONamespace>GAZ</oboInOwl:hasOBONamespace>
        <oboInOwl:id>GAZ:00237192</oboInOwl:id>
        <rdfs:label>Ishongororo Sub-county</rdfs:label>
    </owl:NamedIndividual>
    


    <!-- http://purl.obolibrary.org/obo/GAZ_00237193 -->

    <owl:NamedIndividual rdf:about="http://purl.obolibrary.org/obo/GAZ_00237193">
        <obo:IAO_0000115>A fourth-level administrative division of Uganda.</obo:IAO_0000115>
        <oboInOwl:hasOBONamespace>GAZ</oboInOwl:hasOBONamespace>
        <oboInOwl:id>GAZ:00237193</oboInOwl:id>
        <rdfs:label>Kicuzi Sub-county</rdfs:label>
    </owl:NamedIndividual>
    


    <!-- http://purl.obolibrary.org/obo/GAZ_00237194 -->

    <owl:NamedIndividual rdf:about="http://purl.obolibrary.org/obo/GAZ_00237194">
        <obo:IAO_0000115>A fourth-level administrative division of Uganda.</obo:IAO_0000115>
        <oboInOwl:hasOBONamespace>GAZ</oboInOwl:hasOBONamespace>
        <oboInOwl:id>GAZ:00237194</oboInOwl:id>
        <rdfs:label>Kikyenkye Sub-county</rdfs:label>
    </owl:NamedIndividual>
    


    <!-- http://purl.obolibrary.org/obo/GAZ_00237195 -->

    <owl:NamedIndividual rdf:about="http://purl.obolibrary.org/obo/GAZ_00237195">
        <obo:IAO_0000115>A fourth-level administrative division of Uganda.</obo:IAO_0000115>
        <oboInOwl:hasOBONamespace>GAZ</oboInOwl:hasOBONamespace>
        <oboInOwl:id>GAZ:00237195</oboInOwl:id>
        <rdfs:label>Nyabuhikye Sub-county</rdfs:label>
    </owl:NamedIndividual>
    


    <!-- http://purl.obolibrary.org/obo/GAZ_00237196 -->

    <owl:NamedIndividual rdf:about="http://purl.obolibrary.org/obo/GAZ_00237196">
        <obo:IAO_0000115>A fourth-level administrative division of Uganda.</obo:IAO_0000115>
        <oboInOwl:hasOBONamespace>GAZ</oboInOwl:hasOBONamespace>
        <oboInOwl:id>GAZ:00237196</oboInOwl:id>
        <rdfs:label>Nyamarebe Sub-county</rdfs:label>
    </owl:NamedIndividual>
    


    <!-- http://purl.obolibrary.org/obo/GAZ_00237197 -->

    <owl:NamedIndividual rdf:about="http://purl.obolibrary.org/obo/GAZ_00237197">
        <obo:IAO_0000115>A fourth-level administrative division of Uganda.</obo:IAO_0000115>
        <oboInOwl:hasOBONamespace>GAZ</oboInOwl:hasOBONamespace>
        <oboInOwl:id>GAZ:00237197</oboInOwl:id>
        <rdfs:label>Rukiri Sub-county</rdfs:label>
    </owl:NamedIndividual>
    


    <!-- http://purl.obolibrary.org/obo/GAZ_00237199 -->

    <owl:NamedIndividual rdf:about="http://purl.obolibrary.org/obo/GAZ_00237199">
        <obo:IAO_0000115>A fourth-level administrative division of Uganda.</obo:IAO_0000115>
        <oboInOwl:hasOBONamespace>GAZ</oboInOwl:hasOBONamespace>
        <oboInOwl:id>GAZ:00237199</oboInOwl:id>
        <rdfs:label>Birere Sub-county</rdfs:label>
    </owl:NamedIndividual>
    


    <!-- http://purl.obolibrary.org/obo/GAZ_00237200 -->

    <owl:NamedIndividual rdf:about="http://purl.obolibrary.org/obo/GAZ_00237200">
        <obo:IAO_0000115>A fourth-level administrative division of Uganda.</obo:IAO_0000115>
        <oboInOwl:hasOBONamespace>GAZ</oboInOwl:hasOBONamespace>
        <oboInOwl:id>GAZ:00237200</oboInOwl:id>
        <rdfs:label>Kabingo Sub-county</rdfs:label>
    </owl:NamedIndividual>
    


    <!-- http://purl.obolibrary.org/obo/GAZ_00237201 -->

    <owl:NamedIndividual rdf:about="http://purl.obolibrary.org/obo/GAZ_00237201">
        <obo:IAO_0000115>A fourth-level administrative division of Uganda.</obo:IAO_0000115>
        <oboInOwl:hasOBONamespace>GAZ</oboInOwl:hasOBONamespace>
        <oboInOwl:id>GAZ:00237201</oboInOwl:id>
        <rdfs:label>Kabuyanda Sub-county</rdfs:label>
    </owl:NamedIndividual>
    


    <!-- http://purl.obolibrary.org/obo/GAZ_00237202 -->

    <owl:NamedIndividual rdf:about="http://purl.obolibrary.org/obo/GAZ_00237202">
        <obo:IAO_0000115>A fourth-level administrative division of Uganda.</obo:IAO_0000115>
        <oboInOwl:hasOBONamespace>GAZ</oboInOwl:hasOBONamespace>
        <oboInOwl:id>GAZ:00237202</oboInOwl:id>
        <rdfs:label>Kikagate Sub-county</rdfs:label>
    </owl:NamedIndividual>
    


    <!-- http://purl.obolibrary.org/obo/GAZ_00237203 -->

    <owl:NamedIndividual rdf:about="http://purl.obolibrary.org/obo/GAZ_00237203">
        <obo:IAO_0000115>A fourth-level administrative division of Uganda.</obo:IAO_0000115>
        <oboInOwl:hasOBONamespace>GAZ</oboInOwl:hasOBONamespace>
        <oboInOwl:id>GAZ:00237203</oboInOwl:id>
        <rdfs:label>Masha Sub-county</rdfs:label>
    </owl:NamedIndividual>
    


    <!-- http://purl.obolibrary.org/obo/GAZ_00237204 -->

    <owl:NamedIndividual rdf:about="http://purl.obolibrary.org/obo/GAZ_00237204">
        <obo:IAO_0000115>A fourth-level administrative division of Uganda.</obo:IAO_0000115>
        <oboInOwl:hasOBONamespace>GAZ</oboInOwl:hasOBONamespace>
        <oboInOwl:id>GAZ:00237204</oboInOwl:id>
        <rdfs:label>Nyakitunda Sub-county</rdfs:label>
    </owl:NamedIndividual>
    


    <!-- http://purl.obolibrary.org/obo/GAZ_00237205 -->

    <owl:NamedIndividual rdf:about="http://purl.obolibrary.org/obo/GAZ_00237205">
        <obo:RO_0001025 rdf:resource="http://purl.obolibrary.org/obo/GAZ_00015546"/>
        <obo:IAO_0000115>A fourth-level administrative division of Uganda.</obo:IAO_0000115>
        <oboInOwl:hasOBONamespace>GAZ</oboInOwl:hasOBONamespace>
        <oboInOwl:id>GAZ:00237205</oboInOwl:id>
        <rdfs:label>Kabale Central Division</rdfs:label>
    </owl:NamedIndividual>
    


    <!-- http://purl.obolibrary.org/obo/GAZ_00237206 -->

    <owl:NamedIndividual rdf:about="http://purl.obolibrary.org/obo/GAZ_00237206">
        <obo:RO_0001025 rdf:resource="http://purl.obolibrary.org/obo/GAZ_00015546"/>
        <obo:IAO_0000115>A fourth-level administrative division of Uganda.</obo:IAO_0000115>
        <oboInOwl:hasOBONamespace>GAZ</oboInOwl:hasOBONamespace>
        <oboInOwl:id>GAZ:00237206</oboInOwl:id>
        <rdfs:label>Kabale Northern Division</rdfs:label>
    </owl:NamedIndividual>
    


    <!-- http://purl.obolibrary.org/obo/GAZ_00237207 -->

    <owl:NamedIndividual rdf:about="http://purl.obolibrary.org/obo/GAZ_00237207">
        <obo:RO_0001025 rdf:resource="http://purl.obolibrary.org/obo/GAZ_00015546"/>
        <obo:IAO_0000115>A fourth-level administrative division of Uganda.</obo:IAO_0000115>
        <oboInOwl:hasOBONamespace>GAZ</oboInOwl:hasOBONamespace>
        <oboInOwl:id>GAZ:00237207</oboInOwl:id>
        <rdfs:label>Kabale Southern Division</rdfs:label>
    </owl:NamedIndividual>
    


    <!-- http://purl.obolibrary.org/obo/GAZ_00237208 -->

    <owl:NamedIndividual rdf:about="http://purl.obolibrary.org/obo/GAZ_00237208">
        <obo:RO_0001025 rdf:resource="http://purl.obolibrary.org/obo/GAZ_00015547"/>
        <obo:IAO_0000115>A fourth-level administrative division of Uganda.</obo:IAO_0000115>
        <oboInOwl:hasOBONamespace>GAZ</oboInOwl:hasOBONamespace>
        <oboInOwl:id>GAZ:00237208</oboInOwl:id>
        <rdfs:label>Buhara Sub-county</rdfs:label>
    </owl:NamedIndividual>
    


    <!-- http://purl.obolibrary.org/obo/GAZ_00237209 -->

    <owl:NamedIndividual rdf:about="http://purl.obolibrary.org/obo/GAZ_00237209">
        <obo:RO_0001025 rdf:resource="http://purl.obolibrary.org/obo/GAZ_00015547"/>
        <obo:IAO_0000115>A fourth-level administrative division of Uganda.</obo:IAO_0000115>
        <oboInOwl:hasOBONamespace>GAZ</oboInOwl:hasOBONamespace>
        <oboInOwl:id>GAZ:00237209</oboInOwl:id>
        <rdfs:label>Kaharo Sub-county</rdfs:label>
    </owl:NamedIndividual>
    


    <!-- http://purl.obolibrary.org/obo/GAZ_00237210 -->

    <owl:NamedIndividual rdf:about="http://purl.obolibrary.org/obo/GAZ_00237210">
        <obo:RO_0001025 rdf:resource="http://purl.obolibrary.org/obo/GAZ_00015547"/>
        <obo:IAO_0000115>A fourth-level administrative division of Uganda.</obo:IAO_0000115>
        <oboInOwl:hasOBONamespace>GAZ</oboInOwl:hasOBONamespace>
        <oboInOwl:id>GAZ:00237210</oboInOwl:id>
        <rdfs:label>Kamuganguzi Sub-county</rdfs:label>
    </owl:NamedIndividual>
    


    <!-- http://purl.obolibrary.org/obo/GAZ_00237211 -->

    <owl:NamedIndividual rdf:about="http://purl.obolibrary.org/obo/GAZ_00237211">
        <obo:RO_0001025 rdf:resource="http://purl.obolibrary.org/obo/GAZ_00015547"/>
        <obo:IAO_0000115>A fourth-level administrative division of Uganda.</obo:IAO_0000115>
        <oboInOwl:hasOBONamespace>GAZ</oboInOwl:hasOBONamespace>
        <oboInOwl:id>GAZ:00237211</oboInOwl:id>
        <rdfs:label>Kitumba Sub-county</rdfs:label>
    </owl:NamedIndividual>
    


    <!-- http://purl.obolibrary.org/obo/GAZ_00237212 -->

    <owl:NamedIndividual rdf:about="http://purl.obolibrary.org/obo/GAZ_00237212">
        <obo:RO_0001025 rdf:resource="http://purl.obolibrary.org/obo/GAZ_00015547"/>
        <obo:IAO_0000115>A fourth-level administrative division of Uganda.</obo:IAO_0000115>
        <oboInOwl:hasOBONamespace>GAZ</oboInOwl:hasOBONamespace>
        <oboInOwl:id>GAZ:00237212</oboInOwl:id>
        <rdfs:label>Kyanamira Sub-county</rdfs:label>
    </owl:NamedIndividual>
    


    <!-- http://purl.obolibrary.org/obo/GAZ_00237213 -->

    <owl:NamedIndividual rdf:about="http://purl.obolibrary.org/obo/GAZ_00237213">
        <obo:RO_0001025 rdf:resource="http://purl.obolibrary.org/obo/GAZ_00015547"/>
        <obo:IAO_0000115>A fourth-level administrative division of Uganda.</obo:IAO_0000115>
        <oboInOwl:hasOBONamespace>GAZ</oboInOwl:hasOBONamespace>
        <oboInOwl:id>GAZ:00237213</oboInOwl:id>
        <rdfs:label>Maziba Sub-county</rdfs:label>
    </owl:NamedIndividual>
    


    <!-- http://purl.obolibrary.org/obo/GAZ_00237214 -->

    <owl:NamedIndividual rdf:about="http://purl.obolibrary.org/obo/GAZ_00237214">
        <obo:RO_0001025 rdf:resource="http://purl.obolibrary.org/obo/GAZ_00015547"/>
        <obo:IAO_0000115>A fourth-level administrative division of Uganda.</obo:IAO_0000115>
        <oboInOwl:hasOBONamespace>GAZ</oboInOwl:hasOBONamespace>
        <oboInOwl:id>GAZ:00237214</oboInOwl:id>
        <rdfs:label>Rubaya Sub-county</rdfs:label>
    </owl:NamedIndividual>
    


    <!-- http://purl.obolibrary.org/obo/GAZ_00237215 -->

    <owl:NamedIndividual rdf:about="http://purl.obolibrary.org/obo/GAZ_00237215">
        <obo:RO_0001025 rdf:resource="http://purl.obolibrary.org/obo/GAZ_00015549"/>
        <obo:IAO_0000115>A fourth-level administrative division of Uganda.</obo:IAO_0000115>
        <oboInOwl:hasOBONamespace>GAZ</oboInOwl:hasOBONamespace>
        <oboInOwl:id>GAZ:00237215</oboInOwl:id>
        <rdfs:label>Bubare Sub-county</rdfs:label>
    </owl:NamedIndividual>
    


    <!-- http://purl.obolibrary.org/obo/GAZ_00237216 -->

    <owl:NamedIndividual rdf:about="http://purl.obolibrary.org/obo/GAZ_00237216">
        <obo:RO_0001025 rdf:resource="http://purl.obolibrary.org/obo/GAZ_00015549"/>
        <obo:IAO_0000115>A fourth-level administrative division of Uganda.</obo:IAO_0000115>
        <oboInOwl:hasOBONamespace>GAZ</oboInOwl:hasOBONamespace>
        <oboInOwl:id>GAZ:00237216</oboInOwl:id>
        <rdfs:label>Bufundi Sub-county</rdfs:label>
    </owl:NamedIndividual>
    


    <!-- http://purl.obolibrary.org/obo/GAZ_00237217 -->

    <owl:NamedIndividual rdf:about="http://purl.obolibrary.org/obo/GAZ_00237217">
        <obo:RO_0001025 rdf:resource="http://purl.obolibrary.org/obo/GAZ_00015549"/>
        <obo:IAO_0000115>A fourth-level administrative division of Uganda.</obo:IAO_0000115>
        <oboInOwl:hasOBONamespace>GAZ</oboInOwl:hasOBONamespace>
        <oboInOwl:id>GAZ:00237217</oboInOwl:id>
        <rdfs:label>Hamurwa Sub-county</rdfs:label>
    </owl:NamedIndividual>
    


    <!-- http://purl.obolibrary.org/obo/GAZ_00237218 -->

    <owl:NamedIndividual rdf:about="http://purl.obolibrary.org/obo/GAZ_00237218">
        <obo:RO_0001025 rdf:resource="http://purl.obolibrary.org/obo/GAZ_00015549"/>
        <obo:IAO_0000115>A fourth-level administrative division of Uganda.</obo:IAO_0000115>
        <oboInOwl:hasOBONamespace>GAZ</oboInOwl:hasOBONamespace>
        <oboInOwl:id>GAZ:00237218</oboInOwl:id>
        <rdfs:label>Ikumba Sub-county</rdfs:label>
    </owl:NamedIndividual>
    


    <!-- http://purl.obolibrary.org/obo/GAZ_00237219 -->

    <owl:NamedIndividual rdf:about="http://purl.obolibrary.org/obo/GAZ_00237219">
        <obo:RO_0001025 rdf:resource="http://purl.obolibrary.org/obo/GAZ_00015549"/>
        <obo:IAO_0000115>A fourth-level administrative division of Uganda.</obo:IAO_0000115>
        <oboInOwl:hasOBONamespace>GAZ</oboInOwl:hasOBONamespace>
        <oboInOwl:id>GAZ:00237219</oboInOwl:id>
        <rdfs:label>Muko Sub-county</rdfs:label>
    </owl:NamedIndividual>
    


    <!-- http://purl.obolibrary.org/obo/GAZ_00237220 -->

    <owl:NamedIndividual rdf:about="http://purl.obolibrary.org/obo/GAZ_00237220">
        <obo:RO_0001025 rdf:resource="http://purl.obolibrary.org/obo/GAZ_00015548"/>
        <obo:IAO_0000115>A fourth-level administrative division of Uganda.</obo:IAO_0000115>
        <oboInOwl:hasOBONamespace>GAZ</oboInOwl:hasOBONamespace>
        <oboInOwl:id>GAZ:00237220</oboInOwl:id>
        <rdfs:label>Bukinda Sub-county</rdfs:label>
    </owl:NamedIndividual>
    


    <!-- http://purl.obolibrary.org/obo/GAZ_00237221 -->

    <owl:NamedIndividual rdf:about="http://purl.obolibrary.org/obo/GAZ_00237221">
        <obo:RO_0001025 rdf:resource="http://purl.obolibrary.org/obo/GAZ_00015548"/>
        <obo:IAO_0000115>A fourth-level administrative division of Uganda.</obo:IAO_0000115>
        <oboInOwl:hasOBONamespace>GAZ</oboInOwl:hasOBONamespace>
        <oboInOwl:id>GAZ:00237221</oboInOwl:id>
        <rdfs:label>Kamwezi Sub-county</rdfs:label>
    </owl:NamedIndividual>
    


    <!-- http://purl.obolibrary.org/obo/GAZ_00237222 -->

    <owl:NamedIndividual rdf:about="http://purl.obolibrary.org/obo/GAZ_00237222">
        <obo:RO_0001025 rdf:resource="http://purl.obolibrary.org/obo/GAZ_00015548"/>
        <obo:IAO_0000115>A fourth-level administrative division of Uganda.</obo:IAO_0000115>
        <oboInOwl:hasOBONamespace>GAZ</oboInOwl:hasOBONamespace>
        <oboInOwl:id>GAZ:00237222</oboInOwl:id>
        <rdfs:label>Kashambya Sub-county</rdfs:label>
    </owl:NamedIndividual>
    


    <!-- http://purl.obolibrary.org/obo/GAZ_00237223 -->

    <owl:NamedIndividual rdf:about="http://purl.obolibrary.org/obo/GAZ_00237223">
        <obo:RO_0001025 rdf:resource="http://purl.obolibrary.org/obo/GAZ_00015548"/>
        <obo:IAO_0000115>A fourth-level administrative division of Uganda.</obo:IAO_0000115>
        <oboInOwl:hasOBONamespace>GAZ</oboInOwl:hasOBONamespace>
        <oboInOwl:id>GAZ:00237223</oboInOwl:id>
        <rdfs:label>Rwamucucu Sub-county</rdfs:label>
    </owl:NamedIndividual>
    


    <!-- http://purl.obolibrary.org/obo/GAZ_00237224 -->

    <owl:NamedIndividual rdf:about="http://purl.obolibrary.org/obo/GAZ_00237224">
        <obo:RO_0001025 rdf:resource="http://purl.obolibrary.org/obo/GAZ_00015543"/>
        <obo:IAO_0000115>A fourth-level administrative division of Uganda.</obo:IAO_0000115>
        <oboInOwl:hasOBONamespace>GAZ</oboInOwl:hasOBONamespace>
        <oboInOwl:id>GAZ:00237224</oboInOwl:id>
        <rdfs:label>Buheesi Sub-county</rdfs:label>
    </owl:NamedIndividual>
    


    <!-- http://purl.obolibrary.org/obo/GAZ_00237225 -->

    <owl:NamedIndividual rdf:about="http://purl.obolibrary.org/obo/GAZ_00237225">
        <obo:RO_0001025 rdf:resource="http://purl.obolibrary.org/obo/GAZ_00015543"/>
        <obo:IAO_0000115>A fourth-level administrative division of Uganda.</obo:IAO_0000115>
        <oboInOwl:hasOBONamespace>GAZ</oboInOwl:hasOBONamespace>
        <oboInOwl:id>GAZ:00237225</oboInOwl:id>
        <rdfs:label>Kibiito Sub-county</rdfs:label>
    </owl:NamedIndividual>
    


    <!-- http://purl.obolibrary.org/obo/GAZ_00237226 -->

    <owl:NamedIndividual rdf:about="http://purl.obolibrary.org/obo/GAZ_00237226">
        <obo:RO_0001025 rdf:resource="http://purl.obolibrary.org/obo/GAZ_00015543"/>
        <obo:IAO_0000115>A fourth-level administrative division of Uganda.</obo:IAO_0000115>
        <oboInOwl:hasOBONamespace>GAZ</oboInOwl:hasOBONamespace>
        <oboInOwl:id>GAZ:00237226</oboInOwl:id>
        <rdfs:label>Kisomoro Sub-county</rdfs:label>
    </owl:NamedIndividual>
    


    <!-- http://purl.obolibrary.org/obo/GAZ_00237227 -->

    <owl:NamedIndividual rdf:about="http://purl.obolibrary.org/obo/GAZ_00237227">
        <obo:RO_0001025 rdf:resource="http://purl.obolibrary.org/obo/GAZ_00015543"/>
        <obo:IAO_0000115>A fourth-level administrative division of Uganda.</obo:IAO_0000115>
        <oboInOwl:hasOBONamespace>GAZ</oboInOwl:hasOBONamespace>
        <oboInOwl:id>GAZ:00237227</oboInOwl:id>
        <rdfs:label>Rwiimi Sub-county</rdfs:label>
    </owl:NamedIndividual>
    


    <!-- http://purl.obolibrary.org/obo/GAZ_00237228 -->

    <owl:NamedIndividual rdf:about="http://purl.obolibrary.org/obo/GAZ_00237228">
        <obo:RO_0001025 rdf:resource="http://purl.obolibrary.org/obo/GAZ_00015544"/>
        <obo:IAO_0000115>A fourth-level administrative division of Uganda.</obo:IAO_0000115>
        <oboInOwl:hasOBONamespace>GAZ</oboInOwl:hasOBONamespace>
        <oboInOwl:id>GAZ:00237228</oboInOwl:id>
        <rdfs:label>Bukuku Sub-county</rdfs:label>
    </owl:NamedIndividual>
    


    <!-- http://purl.obolibrary.org/obo/GAZ_00237229 -->

    <owl:NamedIndividual rdf:about="http://purl.obolibrary.org/obo/GAZ_00237229">
        <obo:RO_0001025 rdf:resource="http://purl.obolibrary.org/obo/GAZ_00015544"/>
        <obo:IAO_0000115>A fourth-level administrative division of Uganda.</obo:IAO_0000115>
        <oboInOwl:hasOBONamespace>GAZ</oboInOwl:hasOBONamespace>
        <oboInOwl:id>GAZ:00237229</oboInOwl:id>
        <rdfs:label>Busoro Sub-county</rdfs:label>
    </owl:NamedIndividual>
    


    <!-- http://purl.obolibrary.org/obo/GAZ_00237230 -->

    <owl:NamedIndividual rdf:about="http://purl.obolibrary.org/obo/GAZ_00237230">
        <obo:RO_0001025 rdf:resource="http://purl.obolibrary.org/obo/GAZ_00015544"/>
        <obo:IAO_0000115>A fourth-level administrative division of Uganda.</obo:IAO_0000115>
        <oboInOwl:hasOBONamespace>GAZ</oboInOwl:hasOBONamespace>
        <oboInOwl:id>GAZ:00237230</oboInOwl:id>
        <rdfs:label>Hakibaale Sub-county</rdfs:label>
    </owl:NamedIndividual>
    


    <!-- http://purl.obolibrary.org/obo/GAZ_00237231 -->

    <owl:NamedIndividual rdf:about="http://purl.obolibrary.org/obo/GAZ_00237231">
        <obo:RO_0001025 rdf:resource="http://purl.obolibrary.org/obo/GAZ_00015544"/>
        <obo:IAO_0000115>A fourth-level administrative division of Uganda.</obo:IAO_0000115>
        <oboInOwl:hasOBONamespace>GAZ</oboInOwl:hasOBONamespace>
        <oboInOwl:id>GAZ:00237231</oboInOwl:id>
        <rdfs:label>Karambi Sub-county</rdfs:label>
    </owl:NamedIndividual>
    


    <!-- http://purl.obolibrary.org/obo/GAZ_00237232 -->

    <owl:NamedIndividual rdf:about="http://purl.obolibrary.org/obo/GAZ_00237232">
        <obo:RO_0001025 rdf:resource="http://purl.obolibrary.org/obo/GAZ_00015544"/>
        <obo:IAO_0000115>A fourth-level administrative division of Uganda.</obo:IAO_0000115>
        <oboInOwl:hasOBONamespace>GAZ</oboInOwl:hasOBONamespace>
        <oboInOwl:id>GAZ:00237232</oboInOwl:id>
        <rdfs:label>Kicwamba Sub-county</rdfs:label>
    </owl:NamedIndividual>
    


    <!-- http://purl.obolibrary.org/obo/GAZ_00237233 -->

    <owl:NamedIndividual rdf:about="http://purl.obolibrary.org/obo/GAZ_00237233">
        <obo:RO_0001025 rdf:resource="http://purl.obolibrary.org/obo/GAZ_00015544"/>
        <obo:IAO_0000115>A fourth-level administrative division of Uganda.</obo:IAO_0000115>
        <oboInOwl:hasOBONamespace>GAZ</oboInOwl:hasOBONamespace>
        <oboInOwl:id>GAZ:00237233</oboInOwl:id>
        <rdfs:label>Mugusu Sub-county</rdfs:label>
    </owl:NamedIndividual>
    


    <!-- http://purl.obolibrary.org/obo/GAZ_00237234 -->

    <owl:NamedIndividual rdf:about="http://purl.obolibrary.org/obo/GAZ_00237234">
        <obo:RO_0001025 rdf:resource="http://purl.obolibrary.org/obo/GAZ_00015544"/>
        <obo:IAO_0000115>A fourth-level administrative division of Uganda.</obo:IAO_0000115>
        <oboInOwl:hasOBONamespace>GAZ</oboInOwl:hasOBONamespace>
        <oboInOwl:id>GAZ:00237234</oboInOwl:id>
        <rdfs:label>Ruteete Sub-county</rdfs:label>
    </owl:NamedIndividual>
    


    <!-- http://purl.obolibrary.org/obo/GAZ_00237235 -->

    <owl:NamedIndividual rdf:about="http://purl.obolibrary.org/obo/GAZ_00237235">
        <obo:RO_0001025 rdf:resource="http://purl.obolibrary.org/obo/GAZ_00015545"/>
        <obo:IAO_0000115>A fourth-level administrative division of Uganda.</obo:IAO_0000115>
        <oboInOwl:hasOBONamespace>GAZ</oboInOwl:hasOBONamespace>
        <oboInOwl:id>GAZ:00237235</oboInOwl:id>
        <rdfs:label>Fort Portal Eastern Division</rdfs:label>
    </owl:NamedIndividual>
    


    <!-- http://purl.obolibrary.org/obo/GAZ_00237236 -->

    <owl:NamedIndividual rdf:about="http://purl.obolibrary.org/obo/GAZ_00237236">
        <obo:RO_0001025 rdf:resource="http://purl.obolibrary.org/obo/GAZ_00015545"/>
        <obo:IAO_0000115>A fourth-level administrative division of Uganda.</obo:IAO_0000115>
        <oboInOwl:hasOBONamespace>GAZ</oboInOwl:hasOBONamespace>
        <oboInOwl:id>GAZ:00237236</oboInOwl:id>
        <rdfs:label>Fort Portal Western Division</rdfs:label>
    </owl:NamedIndividual>
    


    <!-- http://purl.obolibrary.org/obo/GAZ_00237237 -->

    <owl:NamedIndividual rdf:about="http://purl.obolibrary.org/obo/GAZ_00237237">
        <obo:RO_0001025 rdf:resource="http://purl.obolibrary.org/obo/GAZ_00015545"/>
        <obo:IAO_0000115>A fourth-level administrative division of Uganda.</obo:IAO_0000115>
        <oboInOwl:hasOBONamespace>GAZ</oboInOwl:hasOBONamespace>
        <oboInOwl:id>GAZ:00237237</oboInOwl:id>
        <rdfs:label>Fort Portal Southern Division</rdfs:label>
    </owl:NamedIndividual>
    


    <!-- http://purl.obolibrary.org/obo/GAZ_00237238 -->

    <owl:NamedIndividual rdf:about="http://purl.obolibrary.org/obo/GAZ_00237238">
        <obo:RO_0001025 rdf:resource="http://purl.obolibrary.org/obo/GAZ_00015541"/>
        <obo:IAO_0000115>A fourth-level administrative division of Uganda.</obo:IAO_0000115>
        <oboInOwl:hasOBONamespace>GAZ</oboInOwl:hasOBONamespace>
        <oboInOwl:id>GAZ:00237238</oboInOwl:id>
        <rdfs:label>Bwiizi Sub-county</rdfs:label>
    </owl:NamedIndividual>
    


    <!-- http://purl.obolibrary.org/obo/GAZ_00237239 -->

    <owl:NamedIndividual rdf:about="http://purl.obolibrary.org/obo/GAZ_00237239">
        <obo:RO_0001025 rdf:resource="http://purl.obolibrary.org/obo/GAZ_00015541"/>
        <obo:IAO_0000115>A fourth-level administrative division of Uganda.</obo:IAO_0000115>
        <oboInOwl:hasOBONamespace>GAZ</oboInOwl:hasOBONamespace>
        <oboInOwl:id>GAZ:00237239</oboInOwl:id>
        <rdfs:label>Kahunge Sub-county</rdfs:label>
    </owl:NamedIndividual>
    


    <!-- http://purl.obolibrary.org/obo/GAZ_00237240 -->

    <owl:NamedIndividual rdf:about="http://purl.obolibrary.org/obo/GAZ_00237240">
        <obo:RO_0001025 rdf:resource="http://purl.obolibrary.org/obo/GAZ_00015541"/>
        <obo:IAO_0000115>A fourth-level administrative division of Uganda.</obo:IAO_0000115>
        <oboInOwl:hasOBONamespace>GAZ</oboInOwl:hasOBONamespace>
        <oboInOwl:id>GAZ:00237240</oboInOwl:id>
        <rdfs:label>Kamwenge Sub-county</rdfs:label>
    </owl:NamedIndividual>
    


    <!-- http://purl.obolibrary.org/obo/GAZ_00237241 -->

    <owl:NamedIndividual rdf:about="http://purl.obolibrary.org/obo/GAZ_00237241">
        <obo:RO_0001025 rdf:resource="http://purl.obolibrary.org/obo/GAZ_00015541"/>
        <obo:IAO_0000115>A fourth-level administrative division of Uganda.</obo:IAO_0000115>
        <oboInOwl:hasOBONamespace>GAZ</oboInOwl:hasOBONamespace>
        <oboInOwl:id>GAZ:00237241</oboInOwl:id>
        <rdfs:label>Kamwenge Town</rdfs:label>
    </owl:NamedIndividual>
    


    <!-- http://purl.obolibrary.org/obo/GAZ_00237242 -->

    <owl:NamedIndividual rdf:about="http://purl.obolibrary.org/obo/GAZ_00237242">
        <obo:RO_0001025 rdf:resource="http://purl.obolibrary.org/obo/GAZ_00015541"/>
        <obo:IAO_0000115>A fourth-level administrative division of Uganda.</obo:IAO_0000115>
        <oboInOwl:hasOBONamespace>GAZ</oboInOwl:hasOBONamespace>
        <oboInOwl:id>GAZ:00237242</oboInOwl:id>
        <rdfs:label>Nkoma Sub-county</rdfs:label>
    </owl:NamedIndividual>
    


    <!-- http://purl.obolibrary.org/obo/GAZ_00237243 -->

    <owl:NamedIndividual rdf:about="http://purl.obolibrary.org/obo/GAZ_00237243">
        <obo:RO_0001025 rdf:resource="http://purl.obolibrary.org/obo/GAZ_00015542"/>
        <obo:IAO_0000115>A fourth-level administrative division of Uganda.</obo:IAO_0000115>
        <oboInOwl:hasOBONamespace>GAZ</oboInOwl:hasOBONamespace>
        <oboInOwl:id>GAZ:00237243</oboInOwl:id>
        <rdfs:label>Kicheche Sub-county</rdfs:label>
    </owl:NamedIndividual>
    


    <!-- http://purl.obolibrary.org/obo/GAZ_00237244 -->

    <owl:NamedIndividual rdf:about="http://purl.obolibrary.org/obo/GAZ_00237244">
        <obo:RO_0001025 rdf:resource="http://purl.obolibrary.org/obo/GAZ_00015542"/>
        <obo:IAO_0000115>A fourth-level administrative division of Uganda.</obo:IAO_0000115>
        <oboInOwl:hasOBONamespace>GAZ</oboInOwl:hasOBONamespace>
        <oboInOwl:id>GAZ:00237244</oboInOwl:id>
        <rdfs:label>Mahyoro Sub-county</rdfs:label>
    </owl:NamedIndividual>
    


    <!-- http://purl.obolibrary.org/obo/GAZ_00237245 -->

    <owl:NamedIndividual rdf:about="http://purl.obolibrary.org/obo/GAZ_00237245">
        <obo:RO_0001025 rdf:resource="http://purl.obolibrary.org/obo/GAZ_00015542"/>
        <obo:IAO_0000115>A fourth-level administrative division of Uganda.</obo:IAO_0000115>
        <oboInOwl:hasOBONamespace>GAZ</oboInOwl:hasOBONamespace>
        <oboInOwl:id>GAZ:00237245</oboInOwl:id>
        <rdfs:label>Ntara Sub-county</rdfs:label>
    </owl:NamedIndividual>
    


    <!-- http://purl.obolibrary.org/obo/GAZ_00237246 -->

    <owl:NamedIndividual rdf:about="http://purl.obolibrary.org/obo/GAZ_00237246">
        <obo:RO_0001025 rdf:resource="http://purl.obolibrary.org/obo/GAZ_00015542"/>
        <obo:IAO_0000115>A fourth-level administrative division of Uganda.</obo:IAO_0000115>
        <oboInOwl:hasOBONamespace>GAZ</oboInOwl:hasOBONamespace>
        <oboInOwl:id>GAZ:00237246</oboInOwl:id>
        <rdfs:label>Nyabbani Sub-county</rdfs:label>
    </owl:NamedIndividual>
    


    <!-- http://purl.obolibrary.org/obo/GAZ_00237247 -->

    <owl:NamedIndividual rdf:about="http://purl.obolibrary.org/obo/GAZ_00237247">
        <obo:IAO_0000115>A fourth-level administrative division of Uganda.</obo:IAO_0000115>
        <oboInOwl:hasOBONamespace>GAZ</oboInOwl:hasOBONamespace>
        <oboInOwl:id>GAZ:00237247</oboInOwl:id>
        <rdfs:label>Kambuga Sub-county</rdfs:label>
    </owl:NamedIndividual>
    


    <!-- http://purl.obolibrary.org/obo/GAZ_00237248 -->

    <owl:NamedIndividual rdf:about="http://purl.obolibrary.org/obo/GAZ_00237248">
        <obo:IAO_0000115>A fourth-level administrative division of Uganda.</obo:IAO_0000115>
        <oboInOwl:hasOBONamespace>GAZ</oboInOwl:hasOBONamespace>
        <oboInOwl:id>GAZ:00237248</oboInOwl:id>
        <rdfs:label>Kanyantorogo Sub-county</rdfs:label>
    </owl:NamedIndividual>
    


    <!-- http://purl.obolibrary.org/obo/GAZ_00237249 -->

    <owl:NamedIndividual rdf:about="http://purl.obolibrary.org/obo/GAZ_00237249">
        <obo:IAO_0000115>A fourth-level administrative division of Uganda.</obo:IAO_0000115>
        <oboInOwl:hasOBONamespace>GAZ</oboInOwl:hasOBONamespace>
        <oboInOwl:id>GAZ:00237249</oboInOwl:id>
        <rdfs:label>Kayonza Sub-county</rdfs:label>
    </owl:NamedIndividual>
    


    <!-- http://purl.obolibrary.org/obo/GAZ_00237250 -->

    <owl:NamedIndividual rdf:about="http://purl.obolibrary.org/obo/GAZ_00237250">
        <obo:IAO_0000115>A fourth-level administrative division of Uganda.</obo:IAO_0000115>
        <oboInOwl:hasOBONamespace>GAZ</oboInOwl:hasOBONamespace>
        <oboInOwl:id>GAZ:00237250</oboInOwl:id>
        <rdfs:label>Kihiihi Sub-county</rdfs:label>
    </owl:NamedIndividual>
    


    <!-- http://purl.obolibrary.org/obo/GAZ_00237251 -->

    <owl:NamedIndividual rdf:about="http://purl.obolibrary.org/obo/GAZ_00237251">
        <obo:IAO_0000115>A fourth-level administrative division of Uganda.</obo:IAO_0000115>
        <oboInOwl:hasOBONamespace>GAZ</oboInOwl:hasOBONamespace>
        <oboInOwl:id>GAZ:00237251</oboInOwl:id>
        <rdfs:label>Kirima Sub-county</rdfs:label>
    </owl:NamedIndividual>
    


    <!-- http://purl.obolibrary.org/obo/GAZ_00237252 -->

    <owl:NamedIndividual rdf:about="http://purl.obolibrary.org/obo/GAZ_00237252">
        <obo:IAO_0000115>A fourth-level administrative division of Uganda.</obo:IAO_0000115>
        <oboInOwl:hasOBONamespace>GAZ</oboInOwl:hasOBONamespace>
        <oboInOwl:id>GAZ:00237252</oboInOwl:id>
        <rdfs:label>Nyamirama Sub-county</rdfs:label>
    </owl:NamedIndividual>
    


    <!-- http://purl.obolibrary.org/obo/GAZ_00237253 -->

    <owl:NamedIndividual rdf:about="http://purl.obolibrary.org/obo/GAZ_00237253">
        <obo:IAO_0000115>A fourth-level administrative division of Uganda.</obo:IAO_0000115>
        <oboInOwl:hasOBONamespace>GAZ</oboInOwl:hasOBONamespace>
        <oboInOwl:id>GAZ:00237253</oboInOwl:id>
        <rdfs:label>Rugyeyo Sub-county</rdfs:label>
    </owl:NamedIndividual>
    


    <!-- http://purl.obolibrary.org/obo/GAZ_00237254 -->

    <owl:NamedIndividual rdf:about="http://purl.obolibrary.org/obo/GAZ_00237254">
        <obo:IAO_0000115>A fourth-level administrative division of Uganda.</obo:IAO_0000115>
        <oboInOwl:hasOBONamespace>GAZ</oboInOwl:hasOBONamespace>
        <oboInOwl:id>GAZ:00237254</oboInOwl:id>
        <rdfs:label>Rutenga Sub-county</rdfs:label>
    </owl:NamedIndividual>
    


    <!-- http://purl.obolibrary.org/obo/GAZ_00237255 -->

    <owl:NamedIndividual rdf:about="http://purl.obolibrary.org/obo/GAZ_00237255">
        <obo:IAO_0000115>A fourth-level administrative division of Uganda.</obo:IAO_0000115>
        <oboInOwl:hasOBONamespace>GAZ</oboInOwl:hasOBONamespace>
        <oboInOwl:id>GAZ:00237255</oboInOwl:id>
        <rdfs:label>Kanungu Town</rdfs:label>
    </owl:NamedIndividual>
    


    <!-- http://purl.obolibrary.org/obo/GAZ_00237256 -->

    <owl:NamedIndividual rdf:about="http://purl.obolibrary.org/obo/GAZ_00237256">
        <obo:IAO_0000115>A fourth-level administrative division of Uganda.</obo:IAO_0000115>
        <oboInOwl:hasOBONamespace>GAZ</oboInOwl:hasOBONamespace>
        <oboInOwl:id>GAZ:00237256</oboInOwl:id>
        <rdfs:label>Mpungu Sub-county</rdfs:label>
    </owl:NamedIndividual>
    


    <!-- http://purl.obolibrary.org/obo/GAZ_00237257 -->

    <owl:NamedIndividual rdf:about="http://purl.obolibrary.org/obo/GAZ_00237257">
        <obo:RO_0001025 rdf:resource="http://purl.obolibrary.org/obo/GAZ_00015410"/>
        <obo:IAO_0000115>A crater lake.</obo:IAO_0000115>
        <oboInOwl:hasOBONamespace>GAZ</oboInOwl:hasOBONamespace>
        <oboInOwl:id>GAZ:00237257</oboInOwl:id>
        <rdfs:label>Lake Mutanda</rdfs:label>
    </owl:NamedIndividual>
    


    <!-- http://purl.obolibrary.org/obo/GAZ_00237258 -->

    <owl:NamedIndividual rdf:about="http://purl.obolibrary.org/obo/GAZ_00237258">
        <obo:RO_0001025 rdf:resource="http://purl.obolibrary.org/obo/GAZ_00015410"/>
        <obo:IAO_0000115>A crater lake.</obo:IAO_0000115>
        <oboInOwl:hasOBONamespace>GAZ</oboInOwl:hasOBONamespace>
        <oboInOwl:id>GAZ:00237258</oboInOwl:id>
        <rdfs:label>Lake Kyahafi</rdfs:label>
    </owl:NamedIndividual>
    


    <!-- http://purl.obolibrary.org/obo/GAZ_00237259 -->

    <owl:NamedIndividual rdf:about="http://purl.obolibrary.org/obo/GAZ_00237259">
        <obo:RO_0001025 rdf:resource="http://purl.obolibrary.org/obo/GAZ_00015408"/>
        <obo:IAO_0000115>Hot springs.</obo:IAO_0000115>
        <oboInOwl:hasOBONamespace>GAZ</oboInOwl:hasOBONamespace>
        <oboInOwl:id>GAZ:00237259</oboInOwl:id>
        <rdfs:label>Nyamasizi Hot Springs</rdfs:label>
    </owl:NamedIndividual>
    


    <!-- http://purl.obolibrary.org/obo/GAZ_00237260 -->

    <owl:NamedIndividual rdf:about="http://purl.obolibrary.org/obo/GAZ_00237260">
        <obo:RO_0001025 rdf:resource="http://purl.obolibrary.org/obo/GAZ_00015538"/>
        <obo:IAO_0000115>A fourth-level administrative division of Uganda.</obo:IAO_0000115>
        <oboInOwl:hasOBONamespace>GAZ</oboInOwl:hasOBONamespace>
        <oboInOwl:id>GAZ:00237260</oboInOwl:id>
        <rdfs:label>Bwera Sub-County</rdfs:label>
    </owl:NamedIndividual>
    


    <!-- http://purl.obolibrary.org/obo/GAZ_00237261 -->

    <owl:NamedIndividual rdf:about="http://purl.obolibrary.org/obo/GAZ_00237261">
        <obo:RO_0001025 rdf:resource="http://purl.obolibrary.org/obo/GAZ_00015538"/>
        <obo:IAO_0000115>A fourth-level administrative division of Uganda.</obo:IAO_0000115>
        <oboInOwl:hasOBONamespace>GAZ</oboInOwl:hasOBONamespace>
        <oboInOwl:id>GAZ:00237261</oboInOwl:id>
        <rdfs:label>Ihandiro Sub-County</rdfs:label>
    </owl:NamedIndividual>
    


    <!-- http://purl.obolibrary.org/obo/GAZ_00237262 -->

    <owl:NamedIndividual rdf:about="http://purl.obolibrary.org/obo/GAZ_00237262">
        <obo:RO_0001025 rdf:resource="http://purl.obolibrary.org/obo/GAZ_00015538"/>
        <obo:IAO_0000115>A fourth-level administrative division of Uganda.</obo:IAO_0000115>
        <oboInOwl:hasOBONamespace>GAZ</oboInOwl:hasOBONamespace>
        <oboInOwl:id>GAZ:00237262</oboInOwl:id>
        <rdfs:label>Karambi Sub-County</rdfs:label>
    </owl:NamedIndividual>
    


    <!-- http://purl.obolibrary.org/obo/GAZ_00237263 -->

    <owl:NamedIndividual rdf:about="http://purl.obolibrary.org/obo/GAZ_00237263">
        <obo:RO_0001025 rdf:resource="http://purl.obolibrary.org/obo/GAZ_00015538"/>
        <obo:IAO_0000115>A fourth-level administrative division of Uganda.</obo:IAO_0000115>
        <oboInOwl:hasOBONamespace>GAZ</oboInOwl:hasOBONamespace>
        <oboInOwl:id>GAZ:00237263</oboInOwl:id>
        <rdfs:label>Kisinga Sub-County</rdfs:label>
    </owl:NamedIndividual>
    


    <!-- http://purl.obolibrary.org/obo/GAZ_00237264 -->

    <owl:NamedIndividual rdf:about="http://purl.obolibrary.org/obo/GAZ_00237264">
        <obo:RO_0001025 rdf:resource="http://purl.obolibrary.org/obo/GAZ_00015538"/>
        <obo:IAO_0000115>A fourth-level administrative division of Uganda.</obo:IAO_0000115>
        <oboInOwl:hasOBONamespace>GAZ</oboInOwl:hasOBONamespace>
        <oboInOwl:id>GAZ:00237264</oboInOwl:id>
        <rdfs:label>Kitholhu Sub-County</rdfs:label>
    </owl:NamedIndividual>
    


    <!-- http://purl.obolibrary.org/obo/GAZ_00237265 -->

    <owl:NamedIndividual rdf:about="http://purl.obolibrary.org/obo/GAZ_00237265">
        <obo:RO_0001025 rdf:resource="http://purl.obolibrary.org/obo/GAZ_00015538"/>
        <obo:IAO_0000115>A fourth-level administrative division of Uganda.</obo:IAO_0000115>
        <oboInOwl:hasOBONamespace>GAZ</oboInOwl:hasOBONamespace>
        <oboInOwl:id>GAZ:00237265</oboInOwl:id>
        <rdfs:label>Kyarumba Sub-County</rdfs:label>
    </owl:NamedIndividual>
    


    <!-- http://purl.obolibrary.org/obo/GAZ_00237266 -->

    <owl:NamedIndividual rdf:about="http://purl.obolibrary.org/obo/GAZ_00237266">
        <obo:RO_0001025 rdf:resource="http://purl.obolibrary.org/obo/GAZ_00015538"/>
        <obo:IAO_0000115>A fourth-level administrative division of Uganda.</obo:IAO_0000115>
        <oboInOwl:hasOBONamespace>GAZ</oboInOwl:hasOBONamespace>
        <oboInOwl:id>GAZ:00237266</oboInOwl:id>
        <rdfs:label>Kyondo Sub-County</rdfs:label>
    </owl:NamedIndividual>
    


    <!-- http://purl.obolibrary.org/obo/GAZ_00237267 -->

    <owl:NamedIndividual rdf:about="http://purl.obolibrary.org/obo/GAZ_00237267">
        <obo:RO_0001025 rdf:resource="http://purl.obolibrary.org/obo/GAZ_00015538"/>
        <obo:IAO_0000115>A fourth-level administrative division of Uganda.</obo:IAO_0000115>
        <oboInOwl:hasOBONamespace>GAZ</oboInOwl:hasOBONamespace>
        <oboInOwl:id>GAZ:00237267</oboInOwl:id>
        <rdfs:label>Mahango Sub-County</rdfs:label>
    </owl:NamedIndividual>
    


    <!-- http://purl.obolibrary.org/obo/GAZ_00237268 -->

    <owl:NamedIndividual rdf:about="http://purl.obolibrary.org/obo/GAZ_00237268">
        <obo:RO_0001025 rdf:resource="http://purl.obolibrary.org/obo/GAZ_00015538"/>
        <obo:IAO_0000115>A fourth-level administrative division of Uganda.</obo:IAO_0000115>
        <oboInOwl:hasOBONamespace>GAZ</oboInOwl:hasOBONamespace>
        <oboInOwl:id>GAZ:00237268</oboInOwl:id>
        <rdfs:label>Munkunyu Sub-County</rdfs:label>
    </owl:NamedIndividual>
    


    <!-- http://purl.obolibrary.org/obo/GAZ_00237269 -->

    <owl:NamedIndividual rdf:about="http://purl.obolibrary.org/obo/GAZ_00237269">
        <obo:RO_0001025 rdf:resource="http://purl.obolibrary.org/obo/GAZ_00015538"/>
        <obo:IAO_0000115>A fourth-level administrative division of Uganda.</obo:IAO_0000115>
        <oboInOwl:hasOBONamespace>GAZ</oboInOwl:hasOBONamespace>
        <oboInOwl:id>GAZ:00237269</oboInOwl:id>
        <rdfs:label>Nyakiyumbu Sub-County</rdfs:label>
    </owl:NamedIndividual>
    


    <!-- http://purl.obolibrary.org/obo/GAZ_00237270 -->

    <owl:NamedIndividual rdf:about="http://purl.obolibrary.org/obo/GAZ_00237270">
        <obo:RO_0001025 rdf:resource="http://purl.obolibrary.org/obo/GAZ_00015539"/>
        <obo:IAO_0000115>A fourth-level administrative division of Uganda.</obo:IAO_0000115>
        <oboInOwl:hasOBONamespace>GAZ</oboInOwl:hasOBONamespace>
        <oboInOwl:id>GAZ:00237270</oboInOwl:id>
        <rdfs:label>Bugoye Sub-county</rdfs:label>
    </owl:NamedIndividual>
    


    <!-- http://purl.obolibrary.org/obo/GAZ_00237271 -->

    <owl:NamedIndividual rdf:about="http://purl.obolibrary.org/obo/GAZ_00237271">
        <obo:RO_0001025 rdf:resource="http://purl.obolibrary.org/obo/GAZ_00015539"/>
        <obo:IAO_0000115>A fourth-level administrative division of Uganda.</obo:IAO_0000115>
        <oboInOwl:hasOBONamespace>GAZ</oboInOwl:hasOBONamespace>
        <oboInOwl:id>GAZ:00237271</oboInOwl:id>
        <rdfs:label>Karusandara Sub-county</rdfs:label>
    </owl:NamedIndividual>
    


    <!-- http://purl.obolibrary.org/obo/GAZ_00237272 -->

    <owl:NamedIndividual rdf:about="http://purl.obolibrary.org/obo/GAZ_00237272">
        <obo:RO_0001025 rdf:resource="http://purl.obolibrary.org/obo/GAZ_00015539"/>
        <obo:IAO_0000115>A fourth-level administrative division of Uganda.</obo:IAO_0000115>
        <oboInOwl:hasOBONamespace>GAZ</oboInOwl:hasOBONamespace>
        <oboInOwl:id>GAZ:00237272</oboInOwl:id>
        <rdfs:label>Kasese Town</rdfs:label>
    </owl:NamedIndividual>
    


    <!-- http://purl.obolibrary.org/obo/GAZ_00237273 -->

    <owl:NamedIndividual rdf:about="http://purl.obolibrary.org/obo/GAZ_00237273">
        <obo:RO_0001025 rdf:resource="http://purl.obolibrary.org/obo/GAZ_00015539"/>
        <obo:IAO_0000115>A fourth-level administrative division of Uganda.</obo:IAO_0000115>
        <oboInOwl:hasOBONamespace>GAZ</oboInOwl:hasOBONamespace>
        <oboInOwl:id>GAZ:00237273</oboInOwl:id>
        <rdfs:label>Katwe Kabatoro Town</rdfs:label>
    </owl:NamedIndividual>
    


    <!-- http://purl.obolibrary.org/obo/GAZ_00237274 -->

    <owl:NamedIndividual rdf:about="http://purl.obolibrary.org/obo/GAZ_00237274">
        <obo:RO_0001025 rdf:resource="http://purl.obolibrary.org/obo/GAZ_00015539"/>
        <obo:IAO_0000115>A fourth-level administrative division of Uganda.</obo:IAO_0000115>
        <oboInOwl:hasOBONamespace>GAZ</oboInOwl:hasOBONamespace>
        <oboInOwl:id>GAZ:00237274</oboInOwl:id>
        <rdfs:label>Kilembe Sub-county</rdfs:label>
    </owl:NamedIndividual>
    


    <!-- http://purl.obolibrary.org/obo/GAZ_00237275 -->

    <owl:NamedIndividual rdf:about="http://purl.obolibrary.org/obo/GAZ_00237275">
        <obo:RO_0001025 rdf:resource="http://purl.obolibrary.org/obo/GAZ_00015539"/>
        <obo:IAO_0000115>A fourth-level administrative division of Uganda.</obo:IAO_0000115>
        <oboInOwl:hasOBONamespace>GAZ</oboInOwl:hasOBONamespace>
        <oboInOwl:id>GAZ:00237275</oboInOwl:id>
        <rdfs:label>Kitswamba Sub-county</rdfs:label>
    </owl:NamedIndividual>
    


    <!-- http://purl.obolibrary.org/obo/GAZ_00237276 -->

    <owl:NamedIndividual rdf:about="http://purl.obolibrary.org/obo/GAZ_00237276">
        <obo:RO_0001025 rdf:resource="http://purl.obolibrary.org/obo/GAZ_00015539"/>
        <obo:IAO_0000115>A fourth-level administrative division of Uganda.</obo:IAO_0000115>
        <oboInOwl:hasOBONamespace>GAZ</oboInOwl:hasOBONamespace>
        <oboInOwl:id>GAZ:00237276</oboInOwl:id>
        <rdfs:label>Kyabarungira Sub-county</rdfs:label>
    </owl:NamedIndividual>
    


    <!-- http://purl.obolibrary.org/obo/GAZ_00237277 -->

    <owl:NamedIndividual rdf:about="http://purl.obolibrary.org/obo/GAZ_00237277">
        <obo:RO_0001025 rdf:resource="http://purl.obolibrary.org/obo/GAZ_00015539"/>
        <obo:IAO_0000115>A fourth-level administrative division of Uganda.</obo:IAO_0000115>
        <oboInOwl:hasOBONamespace>GAZ</oboInOwl:hasOBONamespace>
        <oboInOwl:id>GAZ:00237277</oboInOwl:id>
        <rdfs:label>Lake Katwe Sub-county</rdfs:label>
    </owl:NamedIndividual>
    


    <!-- http://purl.obolibrary.org/obo/GAZ_00237278 -->

    <owl:NamedIndividual rdf:about="http://purl.obolibrary.org/obo/GAZ_00237278">
        <obo:RO_0001025 rdf:resource="http://purl.obolibrary.org/obo/GAZ_00015539"/>
        <obo:IAO_0000115>A fourth-level administrative division of Uganda.</obo:IAO_0000115>
        <oboInOwl:hasOBONamespace>GAZ</oboInOwl:hasOBONamespace>
        <oboInOwl:id>GAZ:00237278</oboInOwl:id>
        <rdfs:label>Maliba Sub-county</rdfs:label>
    </owl:NamedIndividual>
    


    <!-- http://purl.obolibrary.org/obo/GAZ_00237279 -->

    <owl:NamedIndividual rdf:about="http://purl.obolibrary.org/obo/GAZ_00237279">
        <obo:RO_0001025 rdf:resource="http://purl.obolibrary.org/obo/GAZ_00015539"/>
        <obo:IAO_0000115>A fourth-level administrative division of Uganda.</obo:IAO_0000115>
        <oboInOwl:hasOBONamespace>GAZ</oboInOwl:hasOBONamespace>
        <oboInOwl:id>GAZ:00237279</oboInOwl:id>
        <rdfs:label>Muhokyax Sub-county</rdfs:label>
    </owl:NamedIndividual>
    


    <!-- http://purl.obolibrary.org/obo/GAZ_00237280 -->

    <owl:NamedIndividual rdf:about="http://purl.obolibrary.org/obo/GAZ_00237280">
        <obo:RO_0001025 rdf:resource="http://purl.obolibrary.org/obo/GAZ_00015539"/>
        <obo:IAO_0000115>A fourth-level administrative division of Uganda.</obo:IAO_0000115>
        <oboInOwl:hasOBONamespace>GAZ</oboInOwl:hasOBONamespace>
        <oboInOwl:id>GAZ:00237280</oboInOwl:id>
        <rdfs:label>Rukoki Sub-county</rdfs:label>
    </owl:NamedIndividual>
    


    <!-- http://purl.obolibrary.org/obo/GAZ_00237281 -->

    <owl:NamedIndividual rdf:about="http://purl.obolibrary.org/obo/GAZ_00237281">
        <obo:RO_0001025 rdf:resource="http://purl.obolibrary.org/obo/GAZ_00237277"/>
        <obo:IAO_0000115>A saline lake.</obo:IAO_0000115>
        <oboInOwl:hasOBONamespace>GAZ</oboInOwl:hasOBONamespace>
        <oboInOwl:id>GAZ:00237281</oboInOwl:id>
        <rdfs:label>Lake Katwe</rdfs:label>
    </owl:NamedIndividual>
    


    <!-- http://purl.obolibrary.org/obo/GAZ_00237282 -->

    <owl:NamedIndividual rdf:about="http://purl.obolibrary.org/obo/GAZ_00237282">
        <obo:RO_0001025 rdf:resource="http://purl.obolibrary.org/obo/GAZ_00015535"/>
        <obo:IAO_0000115>A fourth-level administrative division of Uganda.</obo:IAO_0000115>
        <oboInOwl:hasOBONamespace>GAZ</oboInOwl:hasOBONamespace>
        <oboInOwl:id>GAZ:00237282</oboInOwl:id>
        <rdfs:label>Bwanswa Sub-county</rdfs:label>
    </owl:NamedIndividual>
    


    <!-- http://purl.obolibrary.org/obo/GAZ_00237283 -->

    <owl:NamedIndividual rdf:about="http://purl.obolibrary.org/obo/GAZ_00237283">
        <obo:RO_0001025 rdf:resource="http://purl.obolibrary.org/obo/GAZ_00015535"/>
        <obo:IAO_0000115>A fourth-level administrative division of Uganda.</obo:IAO_0000115>
        <oboInOwl:hasOBONamespace>GAZ</oboInOwl:hasOBONamespace>
        <oboInOwl:id>GAZ:00237283</oboInOwl:id>
        <rdfs:label>Kakindo Sub-county</rdfs:label>
    </owl:NamedIndividual>
    


    <!-- http://purl.obolibrary.org/obo/GAZ_00237284 -->

    <owl:NamedIndividual rdf:about="http://purl.obolibrary.org/obo/GAZ_00237284">
        <obo:RO_0001025 rdf:resource="http://purl.obolibrary.org/obo/GAZ_00015535"/>
        <obo:IAO_0000115>A fourth-level administrative division of Uganda.</obo:IAO_0000115>
        <oboInOwl:hasOBONamespace>GAZ</oboInOwl:hasOBONamespace>
        <oboInOwl:id>GAZ:00237284</oboInOwl:id>
        <rdfs:label>Kasambya Sub-county</rdfs:label>
    </owl:NamedIndividual>
    


    <!-- http://purl.obolibrary.org/obo/GAZ_00237285 -->

    <owl:NamedIndividual rdf:about="http://purl.obolibrary.org/obo/GAZ_00237285">
        <obo:RO_0001025 rdf:resource="http://purl.obolibrary.org/obo/GAZ_00015535"/>
        <obo:IAO_0000115>A fourth-level administrative division of Uganda.</obo:IAO_0000115>
        <oboInOwl:hasOBONamespace>GAZ</oboInOwl:hasOBONamespace>
        <oboInOwl:id>GAZ:00237285</oboInOwl:id>
        <rdfs:label>Kisiita Sub-county</rdfs:label>
    </owl:NamedIndividual>
    


    <!-- http://purl.obolibrary.org/obo/GAZ_00237286 -->

    <owl:NamedIndividual rdf:about="http://purl.obolibrary.org/obo/GAZ_00237286">
        <obo:RO_0001025 rdf:resource="http://purl.obolibrary.org/obo/GAZ_00015535"/>
        <obo:IAO_0000115>A fourth-level administrative division of Uganda.</obo:IAO_0000115>
        <oboInOwl:hasOBONamespace>GAZ</oboInOwl:hasOBONamespace>
        <oboInOwl:id>GAZ:00237286</oboInOwl:id>
        <rdfs:label>Nalweyo Sub-county</rdfs:label>
    </owl:NamedIndividual>
    


    <!-- http://purl.obolibrary.org/obo/GAZ_00237287 -->

    <owl:NamedIndividual rdf:about="http://purl.obolibrary.org/obo/GAZ_00237287">
        <obo:RO_0001025 rdf:resource="http://purl.obolibrary.org/obo/GAZ_00015535"/>
        <obo:IAO_0000115>A fourth-level administrative division of Uganda.</obo:IAO_0000115>
        <oboInOwl:hasOBONamespace>GAZ</oboInOwl:hasOBONamespace>
        <oboInOwl:id>GAZ:00237287</oboInOwl:id>
        <rdfs:label>Nkooko Sub-county</rdfs:label>
    </owl:NamedIndividual>
    


    <!-- http://purl.obolibrary.org/obo/GAZ_00237288 -->

    <owl:NamedIndividual rdf:about="http://purl.obolibrary.org/obo/GAZ_00237288">
        <obo:RO_0001025 rdf:resource="http://purl.obolibrary.org/obo/GAZ_00015536"/>
        <obo:IAO_0000115>A fourth-level administrative division of Uganda.</obo:IAO_0000115>
        <oboInOwl:hasOBONamespace>GAZ</oboInOwl:hasOBONamespace>
        <oboInOwl:id>GAZ:00237288</oboInOwl:id>
        <rdfs:label>Bwikara Sub-county</rdfs:label>
    </owl:NamedIndividual>
    


    <!-- http://purl.obolibrary.org/obo/GAZ_00237289 -->

    <owl:NamedIndividual rdf:about="http://purl.obolibrary.org/obo/GAZ_00237289">
        <obo:RO_0001025 rdf:resource="http://purl.obolibrary.org/obo/GAZ_00015536"/>
        <obo:IAO_0000115>A fourth-level administrative division of Uganda.</obo:IAO_0000115>
        <oboInOwl:hasOBONamespace>GAZ</oboInOwl:hasOBONamespace>
        <oboInOwl:id>GAZ:00237289</oboInOwl:id>
        <rdfs:label>Kagadi Sub-county</rdfs:label>
    </owl:NamedIndividual>
    


    <!-- http://purl.obolibrary.org/obo/GAZ_00237290 -->

    <owl:NamedIndividual rdf:about="http://purl.obolibrary.org/obo/GAZ_00237290">
        <obo:RO_0001025 rdf:resource="http://purl.obolibrary.org/obo/GAZ_00015536"/>
        <obo:IAO_0000115>A fourth-level administrative division of Uganda.</obo:IAO_0000115>
        <oboInOwl:hasOBONamespace>GAZ</oboInOwl:hasOBONamespace>
        <oboInOwl:id>GAZ:00237290</oboInOwl:id>
        <rdfs:label>Kiryanga Sub-county</rdfs:label>
    </owl:NamedIndividual>
    


    <!-- http://purl.obolibrary.org/obo/GAZ_00237291 -->

    <owl:NamedIndividual rdf:about="http://purl.obolibrary.org/obo/GAZ_00237291">
        <obo:RO_0001025 rdf:resource="http://purl.obolibrary.org/obo/GAZ_00015536"/>
        <obo:IAO_0000115>A fourth-level administrative division of Uganda.</obo:IAO_0000115>
        <oboInOwl:hasOBONamespace>GAZ</oboInOwl:hasOBONamespace>
        <oboInOwl:id>GAZ:00237291</oboInOwl:id>
        <rdfs:label>Kyanaisoke Sub-county</rdfs:label>
    </owl:NamedIndividual>
    


    <!-- http://purl.obolibrary.org/obo/GAZ_00237292 -->

    <owl:NamedIndividual rdf:about="http://purl.obolibrary.org/obo/GAZ_00237292">
        <obo:RO_0001025 rdf:resource="http://purl.obolibrary.org/obo/GAZ_00015536"/>
        <obo:IAO_0000115>A fourth-level administrative division of Uganda.</obo:IAO_0000115>
        <oboInOwl:hasOBONamespace>GAZ</oboInOwl:hasOBONamespace>
        <oboInOwl:id>GAZ:00237292</oboInOwl:id>
        <rdfs:label>Mabaale Sub-county</rdfs:label>
    </owl:NamedIndividual>
    


    <!-- http://purl.obolibrary.org/obo/GAZ_00237293 -->

    <owl:NamedIndividual rdf:about="http://purl.obolibrary.org/obo/GAZ_00237293">
        <obo:RO_0001025 rdf:resource="http://purl.obolibrary.org/obo/GAZ_00015536"/>
        <obo:IAO_0000115>A fourth-level administrative division of Uganda.</obo:IAO_0000115>
        <oboInOwl:hasOBONamespace>GAZ</oboInOwl:hasOBONamespace>
        <oboInOwl:id>GAZ:00237293</oboInOwl:id>
        <rdfs:label>Mpeefu Sub-county</rdfs:label>
    </owl:NamedIndividual>
    


    <!-- http://purl.obolibrary.org/obo/GAZ_00237294 -->

    <owl:NamedIndividual rdf:about="http://purl.obolibrary.org/obo/GAZ_00237294">
        <obo:RO_0001025 rdf:resource="http://purl.obolibrary.org/obo/GAZ_00015536"/>
        <obo:IAO_0000115>A fourth-level administrative division of Uganda.</obo:IAO_0000115>
        <oboInOwl:hasOBONamespace>GAZ</oboInOwl:hasOBONamespace>
        <oboInOwl:id>GAZ:00237294</oboInOwl:id>
        <rdfs:label>Muhoro Sub-county</rdfs:label>
    </owl:NamedIndividual>
    


    <!-- http://purl.obolibrary.org/obo/GAZ_00237295 -->

    <owl:NamedIndividual rdf:about="http://purl.obolibrary.org/obo/GAZ_00237295">
        <obo:RO_0001025 rdf:resource="http://purl.obolibrary.org/obo/GAZ_00015536"/>
        <obo:IAO_0000115>A fourth-level administrative division of Uganda.</obo:IAO_0000115>
        <oboInOwl:hasOBONamespace>GAZ</oboInOwl:hasOBONamespace>
        <oboInOwl:id>GAZ:00237295</oboInOwl:id>
        <rdfs:label>Rugashari Sub-county</rdfs:label>
    </owl:NamedIndividual>
    


    <!-- http://purl.obolibrary.org/obo/GAZ_00237296 -->

    <owl:NamedIndividual rdf:about="http://purl.obolibrary.org/obo/GAZ_00237296">
        <obo:RO_0001025 rdf:resource="http://purl.obolibrary.org/obo/GAZ_00015537"/>
        <obo:IAO_0000115>A fourth-level administrative division of Uganda.</obo:IAO_0000115>
        <oboInOwl:hasOBONamespace>GAZ</oboInOwl:hasOBONamespace>
        <oboInOwl:id>GAZ:00237296</oboInOwl:id>
        <rdfs:label>Bwamiramira Sub-county</rdfs:label>
    </owl:NamedIndividual>
    


    <!-- http://purl.obolibrary.org/obo/GAZ_00237297 -->

    <owl:NamedIndividual rdf:about="http://purl.obolibrary.org/obo/GAZ_00237297">
        <obo:RO_0001025 rdf:resource="http://purl.obolibrary.org/obo/GAZ_00015537"/>
        <obo:IAO_0000115>A fourth-level administrative division of Uganda.</obo:IAO_0000115>
        <oboInOwl:hasOBONamespace>GAZ</oboInOwl:hasOBONamespace>
        <oboInOwl:id>GAZ:00237297</oboInOwl:id>
        <rdfs:label>Kibaale Town</rdfs:label>
    </owl:NamedIndividual>
    


    <!-- http://purl.obolibrary.org/obo/GAZ_00237298 -->

    <owl:NamedIndividual rdf:about="http://purl.obolibrary.org/obo/GAZ_00237298">
        <obo:RO_0001025 rdf:resource="http://purl.obolibrary.org/obo/GAZ_00015537"/>
        <obo:IAO_0000115>A fourth-level administrative division of Uganda.</obo:IAO_0000115>
        <oboInOwl:hasOBONamespace>GAZ</oboInOwl:hasOBONamespace>
        <oboInOwl:id>GAZ:00237298</oboInOwl:id>
        <rdfs:label>Kyebando Sub-county</rdfs:label>
    </owl:NamedIndividual>
    


    <!-- http://purl.obolibrary.org/obo/GAZ_00237299 -->

    <owl:NamedIndividual rdf:about="http://purl.obolibrary.org/obo/GAZ_00237299">
        <obo:RO_0001025 rdf:resource="http://purl.obolibrary.org/obo/GAZ_00015537"/>
        <obo:IAO_0000115>A fourth-level administrative division of Uganda.</obo:IAO_0000115>
        <oboInOwl:hasOBONamespace>GAZ</oboInOwl:hasOBONamespace>
        <oboInOwl:id>GAZ:00237299</oboInOwl:id>
        <rdfs:label>Matale Sub-county</rdfs:label>
    </owl:NamedIndividual>
    


    <!-- http://purl.obolibrary.org/obo/GAZ_00237300 -->

    <owl:NamedIndividual rdf:about="http://purl.obolibrary.org/obo/GAZ_00237300">
        <obo:RO_0001025 rdf:resource="http://purl.obolibrary.org/obo/GAZ_00015537"/>
        <obo:IAO_0000115>A fourth-level administrative division of Uganda.</obo:IAO_0000115>
        <oboInOwl:hasOBONamespace>GAZ</oboInOwl:hasOBONamespace>
        <oboInOwl:id>GAZ:00237300</oboInOwl:id>
        <rdfs:label>Mugarama Sub-county</rdfs:label>
    </owl:NamedIndividual>
    


    <!-- http://purl.obolibrary.org/obo/GAZ_00237301 -->

    <owl:NamedIndividual rdf:about="http://purl.obolibrary.org/obo/GAZ_00237301">
        <obo:RO_0001025 rdf:resource="http://purl.obolibrary.org/obo/GAZ_00015533"/>
        <obo:IAO_0000115>A fourth-level administrative division of Uganda.</obo:IAO_0000115>
        <oboInOwl:hasOBONamespace>GAZ</oboInOwl:hasOBONamespace>
        <oboInOwl:id>GAZ:00237301</oboInOwl:id>
        <rdfs:label>Buremba Sub-county</rdfs:label>
    </owl:NamedIndividual>
    


    <!-- http://purl.obolibrary.org/obo/GAZ_00237302 -->

    <owl:NamedIndividual rdf:about="http://purl.obolibrary.org/obo/GAZ_00237302">
        <obo:RO_0001025 rdf:resource="http://purl.obolibrary.org/obo/GAZ_00015533"/>
        <obo:IAO_0000115>A fourth-level administrative division of Uganda.</obo:IAO_0000115>
        <oboInOwl:hasOBONamespace>GAZ</oboInOwl:hasOBONamespace>
        <oboInOwl:id>GAZ:00237302</oboInOwl:id>
        <rdfs:label>Burunga Sub-county</rdfs:label>
    </owl:NamedIndividual>
    


    <!-- http://purl.obolibrary.org/obo/GAZ_00237303 -->

    <owl:NamedIndividual rdf:about="http://purl.obolibrary.org/obo/GAZ_00237303">
        <obo:RO_0001025 rdf:resource="http://purl.obolibrary.org/obo/GAZ_00015533"/>
        <obo:IAO_0000115>A fourth-level administrative division of Uganda.</obo:IAO_0000115>
        <oboInOwl:hasOBONamespace>GAZ</oboInOwl:hasOBONamespace>
        <oboInOwl:id>GAZ:00237303</oboInOwl:id>
        <rdfs:label>Kanoni Sub-county</rdfs:label>
    </owl:NamedIndividual>
    


    <!-- http://purl.obolibrary.org/obo/GAZ_00237304 -->

    <owl:NamedIndividual rdf:about="http://purl.obolibrary.org/obo/GAZ_00237304">
        <obo:RO_0001025 rdf:resource="http://purl.obolibrary.org/obo/GAZ_00015533"/>
        <obo:IAO_0000115>A fourth-level administrative division of Uganda.</obo:IAO_0000115>
        <oboInOwl:hasOBONamespace>GAZ</oboInOwl:hasOBONamespace>
        <oboInOwl:id>GAZ:00237304</oboInOwl:id>
        <rdfs:label>Kazo Sub-county</rdfs:label>
    </owl:NamedIndividual>
    


    <!-- http://purl.obolibrary.org/obo/GAZ_00237305 -->

    <owl:NamedIndividual rdf:about="http://purl.obolibrary.org/obo/GAZ_00237305">
        <obo:RO_0001025 rdf:resource="http://purl.obolibrary.org/obo/GAZ_00015533"/>
        <obo:IAO_0000115>A fourth-level administrative division of Uganda.</obo:IAO_0000115>
        <oboInOwl:hasOBONamespace>GAZ</oboInOwl:hasOBONamespace>
        <oboInOwl:id>GAZ:00237305</oboInOwl:id>
        <rdfs:label>Rwemikoma Sub-county</rdfs:label>
    </owl:NamedIndividual>
    


    <!-- http://purl.obolibrary.org/obo/GAZ_00237306 -->

    <owl:NamedIndividual rdf:about="http://purl.obolibrary.org/obo/GAZ_00237306">
        <obo:RO_0001025 rdf:resource="http://purl.obolibrary.org/obo/GAZ_00015534"/>
        <obo:IAO_0000115>A fourth-level administrative division of Uganda.</obo:IAO_0000115>
        <oboInOwl:hasOBONamespace>GAZ</oboInOwl:hasOBONamespace>
        <oboInOwl:id>GAZ:00237306</oboInOwl:id>
        <rdfs:label>Kanyaryeru Sub-county</rdfs:label>
    </owl:NamedIndividual>
    


    <!-- http://purl.obolibrary.org/obo/GAZ_00237307 -->

    <owl:NamedIndividual rdf:about="http://purl.obolibrary.org/obo/GAZ_00237307">
        <obo:RO_0001025 rdf:resource="http://purl.obolibrary.org/obo/GAZ_00015534"/>
        <obo:IAO_0000115>A fourth-level administrative division of Uganda.</obo:IAO_0000115>
        <oboInOwl:hasOBONamespace>GAZ</oboInOwl:hasOBONamespace>
        <oboInOwl:id>GAZ:00237307</oboInOwl:id>
        <rdfs:label>Kashongi Sub-county</rdfs:label>
    </owl:NamedIndividual>
    


    <!-- http://purl.obolibrary.org/obo/GAZ_00237308 -->

    <owl:NamedIndividual rdf:about="http://purl.obolibrary.org/obo/GAZ_00237308">
        <obo:RO_0001025 rdf:resource="http://purl.obolibrary.org/obo/GAZ_00015534"/>
        <obo:IAO_0000115>A fourth-level administrative division of Uganda.</obo:IAO_0000115>
        <oboInOwl:hasOBONamespace>GAZ</oboInOwl:hasOBONamespace>
        <oboInOwl:id>GAZ:00237308</oboInOwl:id>
        <rdfs:label>Kenshunga Sub-county</rdfs:label>
    </owl:NamedIndividual>
    


    <!-- http://purl.obolibrary.org/obo/GAZ_00237309 -->

    <owl:NamedIndividual rdf:about="http://purl.obolibrary.org/obo/GAZ_00237309">
        <obo:RO_0001025 rdf:resource="http://purl.obolibrary.org/obo/GAZ_00015534"/>
        <obo:IAO_0000115>A fourth-level administrative division of Uganda.</obo:IAO_0000115>
        <oboInOwl:hasOBONamespace>GAZ</oboInOwl:hasOBONamespace>
        <oboInOwl:id>GAZ:00237309</oboInOwl:id>
        <rdfs:label>Kikatsi Sub-county</rdfs:label>
    </owl:NamedIndividual>
    


    <!-- http://purl.obolibrary.org/obo/GAZ_00237310 -->

    <owl:NamedIndividual rdf:about="http://purl.obolibrary.org/obo/GAZ_00237310">
        <obo:RO_0001025 rdf:resource="http://purl.obolibrary.org/obo/GAZ_00015534"/>
        <obo:IAO_0000115>A fourth-level administrative division of Uganda.</obo:IAO_0000115>
        <oboInOwl:hasOBONamespace>GAZ</oboInOwl:hasOBONamespace>
        <oboInOwl:id>GAZ:00237310</oboInOwl:id>
        <rdfs:label>Kinoni Sub-county</rdfs:label>
    </owl:NamedIndividual>
    


    <!-- http://purl.obolibrary.org/obo/GAZ_00237311 -->

    <owl:NamedIndividual rdf:about="http://purl.obolibrary.org/obo/GAZ_00237311">
        <obo:RO_0001025 rdf:resource="http://purl.obolibrary.org/obo/GAZ_00015534"/>
        <obo:IAO_0000115>A fourth-level administrative division of Uganda.</obo:IAO_0000115>
        <oboInOwl:hasOBONamespace>GAZ</oboInOwl:hasOBONamespace>
        <oboInOwl:id>GAZ:00237311</oboInOwl:id>
        <rdfs:label>Nyakashashara Sub-county</rdfs:label>
    </owl:NamedIndividual>
    


    <!-- http://purl.obolibrary.org/obo/GAZ_00237312 -->

    <owl:NamedIndividual rdf:about="http://purl.obolibrary.org/obo/GAZ_00237312">
        <obo:RO_0001025 rdf:resource="http://purl.obolibrary.org/obo/GAZ_00015534"/>
        <obo:IAO_0000115>A fourth-level administrative division of Uganda.</obo:IAO_0000115>
        <oboInOwl:hasOBONamespace>GAZ</oboInOwl:hasOBONamespace>
        <oboInOwl:id>GAZ:00237312</oboInOwl:id>
        <rdfs:label>Sanga Sub-county</rdfs:label>
    </owl:NamedIndividual>
    


    <!-- http://purl.obolibrary.org/obo/GAZ_00237313 -->

    <owl:NamedIndividual rdf:about="http://purl.obolibrary.org/obo/GAZ_00237313">
        <obo:IAO_0000115>A fourth-level administrative division of Uganda.</obo:IAO_0000115>
        <oboInOwl:hasOBONamespace>GAZ</oboInOwl:hasOBONamespace>
        <oboInOwl:id>GAZ:00237313</oboInOwl:id>
        <rdfs:label>Bukimbiri Sub-county</rdfs:label>
    </owl:NamedIndividual>
    


    <!-- http://purl.obolibrary.org/obo/GAZ_00237314 -->

    <owl:NamedIndividual rdf:about="http://purl.obolibrary.org/obo/GAZ_00237314">
        <obo:IAO_0000115>A fourth-level administrative division of Uganda.</obo:IAO_0000115>
        <oboInOwl:hasOBONamespace>GAZ</oboInOwl:hasOBONamespace>
        <oboInOwl:id>GAZ:00237314</oboInOwl:id>
        <rdfs:label>Busanza Sub-county</rdfs:label>
    </owl:NamedIndividual>
    


    <!-- http://purl.obolibrary.org/obo/GAZ_00237315 -->

    <owl:NamedIndividual rdf:about="http://purl.obolibrary.org/obo/GAZ_00237315">
        <obo:IAO_0000115>A fourth-level administrative division of Uganda.</obo:IAO_0000115>
        <oboInOwl:hasOBONamespace>GAZ</oboInOwl:hasOBONamespace>
        <oboInOwl:id>GAZ:00237315</oboInOwl:id>
        <rdfs:label>Chahi Sub-county</rdfs:label>
    </owl:NamedIndividual>
    


    <!-- http://purl.obolibrary.org/obo/GAZ_00237316 -->

    <owl:NamedIndividual rdf:about="http://purl.obolibrary.org/obo/GAZ_00237316">
        <obo:IAO_0000115>A fourth-level administrative division of Uganda.</obo:IAO_0000115>
        <oboInOwl:hasOBONamespace>GAZ</oboInOwl:hasOBONamespace>
        <oboInOwl:id>GAZ:00237316</oboInOwl:id>
        <rdfs:label>Kanaba Sub-county</rdfs:label>
    </owl:NamedIndividual>
    


    <!-- http://purl.obolibrary.org/obo/GAZ_00237317 -->

    <owl:NamedIndividual rdf:about="http://purl.obolibrary.org/obo/GAZ_00237317">
        <obo:IAO_0000115>A fourth-level administrative division of Uganda.</obo:IAO_0000115>
        <oboInOwl:hasOBONamespace>GAZ</oboInOwl:hasOBONamespace>
        <oboInOwl:id>GAZ:00237317</oboInOwl:id>
        <rdfs:label>Kirundo Sub-county</rdfs:label>
    </owl:NamedIndividual>
    


    <!-- http://purl.obolibrary.org/obo/GAZ_00237318 -->

    <owl:NamedIndividual rdf:about="http://purl.obolibrary.org/obo/GAZ_00237318">
        <obo:IAO_0000115>A fourth-level administrative division of Uganda.</obo:IAO_0000115>
        <oboInOwl:hasOBONamespace>GAZ</oboInOwl:hasOBONamespace>
        <oboInOwl:id>GAZ:00237318</oboInOwl:id>
        <rdfs:label>Kisoro Town</rdfs:label>
    </owl:NamedIndividual>
    


    <!-- http://purl.obolibrary.org/obo/GAZ_00237319 -->

    <owl:NamedIndividual rdf:about="http://purl.obolibrary.org/obo/GAZ_00237319">
        <obo:IAO_0000115>A fourth-level administrative division of Uganda.</obo:IAO_0000115>
        <oboInOwl:hasOBONamespace>GAZ</oboInOwl:hasOBONamespace>
        <oboInOwl:id>GAZ:00237319</oboInOwl:id>
        <rdfs:label>Muramba Sub-county</rdfs:label>
    </owl:NamedIndividual>
    


    <!-- http://purl.obolibrary.org/obo/GAZ_00237320 -->

    <owl:NamedIndividual rdf:about="http://purl.obolibrary.org/obo/GAZ_00237320">
        <obo:IAO_0000115>A fourth-level administrative division of Uganda.</obo:IAO_0000115>
        <oboInOwl:hasOBONamespace>GAZ</oboInOwl:hasOBONamespace>
        <oboInOwl:id>GAZ:00237320</oboInOwl:id>
        <rdfs:label>Murora Sub-county</rdfs:label>
    </owl:NamedIndividual>
    


    <!-- http://purl.obolibrary.org/obo/GAZ_00237321 -->

    <owl:NamedIndividual rdf:about="http://purl.obolibrary.org/obo/GAZ_00237321">
        <obo:IAO_0000115>A fourth-level administrative division of Uganda.</obo:IAO_0000115>
        <oboInOwl:hasOBONamespace>GAZ</oboInOwl:hasOBONamespace>
        <oboInOwl:id>GAZ:00237321</oboInOwl:id>
        <rdfs:label>Nyabwishenya Sub-county</rdfs:label>
    </owl:NamedIndividual>
    


    <!-- http://purl.obolibrary.org/obo/GAZ_00237322 -->

    <owl:NamedIndividual rdf:about="http://purl.obolibrary.org/obo/GAZ_00237322">
        <obo:IAO_0000115>A fourth-level administrative division of Uganda.</obo:IAO_0000115>
        <oboInOwl:hasOBONamespace>GAZ</oboInOwl:hasOBONamespace>
        <oboInOwl:id>GAZ:00237322</oboInOwl:id>
        <rdfs:label>Nyakabande Sub-county</rdfs:label>
    </owl:NamedIndividual>
    


    <!-- http://purl.obolibrary.org/obo/GAZ_00237323 -->

    <owl:NamedIndividual rdf:about="http://purl.obolibrary.org/obo/GAZ_00237323">
        <obo:IAO_0000115>A fourth-level administrative division of Uganda.</obo:IAO_0000115>
        <oboInOwl:hasOBONamespace>GAZ</oboInOwl:hasOBONamespace>
        <oboInOwl:id>GAZ:00237323</oboInOwl:id>
        <rdfs:label>Nyakinama Sub-county</rdfs:label>
    </owl:NamedIndividual>
    


    <!-- http://purl.obolibrary.org/obo/GAZ_00237324 -->

    <owl:NamedIndividual rdf:about="http://purl.obolibrary.org/obo/GAZ_00237324">
        <obo:IAO_0000115>A fourth-level administrative division of Uganda.</obo:IAO_0000115>
        <oboInOwl:hasOBONamespace>GAZ</oboInOwl:hasOBONamespace>
        <oboInOwl:id>GAZ:00237324</oboInOwl:id>
        <rdfs:label>Nyarubuye Sub-county</rdfs:label>
    </owl:NamedIndividual>
    


    <!-- http://purl.obolibrary.org/obo/GAZ_00237325 -->

    <owl:NamedIndividual rdf:about="http://purl.obolibrary.org/obo/GAZ_00237325">
        <obo:IAO_0000115>A fourth-level administrative division of Uganda.</obo:IAO_0000115>
        <oboInOwl:hasOBONamespace>GAZ</oboInOwl:hasOBONamespace>
        <oboInOwl:id>GAZ:00237325</oboInOwl:id>
        <rdfs:label>Nyarusiza Sub-county</rdfs:label>
    </owl:NamedIndividual>
    


    <!-- http://purl.obolibrary.org/obo/GAZ_00237326 -->

    <owl:NamedIndividual rdf:about="http://purl.obolibrary.org/obo/GAZ_00237326">
        <obo:IAO_0000115>A fourth-level administrative division of Uganda.</obo:IAO_0000115>
        <oboInOwl:hasOBONamespace>GAZ</oboInOwl:hasOBONamespace>
        <oboInOwl:id>GAZ:00237326</oboInOwl:id>
        <rdfs:label>Nyundo Sub-county</rdfs:label>
    </owl:NamedIndividual>
    


    <!-- http://purl.obolibrary.org/obo/GAZ_00237327 -->

    <owl:NamedIndividual rdf:about="http://purl.obolibrary.org/obo/GAZ_00237327">
        <obo:RO_0001025 rdf:resource="http://purl.obolibrary.org/obo/GAZ_00015530"/>
        <obo:IAO_0000115>A fourth-level administrative division of Uganda.</obo:IAO_0000115>
        <oboInOwl:hasOBONamespace>GAZ</oboInOwl:hasOBONamespace>
        <oboInOwl:id>GAZ:00237327</oboInOwl:id>
        <rdfs:label>Hapuyo Sub-county</rdfs:label>
    </owl:NamedIndividual>
    


    <!-- http://purl.obolibrary.org/obo/GAZ_00237328 -->

    <owl:NamedIndividual rdf:about="http://purl.obolibrary.org/obo/GAZ_00237328">
        <obo:RO_0001025 rdf:resource="http://purl.obolibrary.org/obo/GAZ_00015530"/>
        <obo:IAO_0000115>A fourth-level administrative division of Uganda.</obo:IAO_0000115>
        <oboInOwl:hasOBONamespace>GAZ</oboInOwl:hasOBONamespace>
        <oboInOwl:id>GAZ:00237328</oboInOwl:id>
        <rdfs:label>Kakabara Sub-county</rdfs:label>
    </owl:NamedIndividual>
    


    <!-- http://purl.obolibrary.org/obo/GAZ_00237329 -->

    <owl:NamedIndividual rdf:about="http://purl.obolibrary.org/obo/GAZ_00237329">
        <obo:RO_0001025 rdf:resource="http://purl.obolibrary.org/obo/GAZ_00015530"/>
        <obo:IAO_0000115>A fourth-level administrative division of Uganda.</obo:IAO_0000115>
        <oboInOwl:hasOBONamespace>GAZ</oboInOwl:hasOBONamespace>
        <oboInOwl:id>GAZ:00237329</oboInOwl:id>
        <rdfs:label>Kasule Sub-county</rdfs:label>
    </owl:NamedIndividual>
    


    <!-- http://purl.obolibrary.org/obo/GAZ_00237330 -->

    <owl:NamedIndividual rdf:about="http://purl.obolibrary.org/obo/GAZ_00237330">
        <obo:RO_0001025 rdf:resource="http://purl.obolibrary.org/obo/GAZ_00015530"/>
        <obo:IAO_0000115>A fourth-level administrative division of Uganda.</obo:IAO_0000115>
        <oboInOwl:hasOBONamespace>GAZ</oboInOwl:hasOBONamespace>
        <oboInOwl:id>GAZ:00237330</oboInOwl:id>
        <rdfs:label>Kyegegwa Sub-county</rdfs:label>
    </owl:NamedIndividual>
    


    <!-- http://purl.obolibrary.org/obo/GAZ_00237331 -->

    <owl:NamedIndividual rdf:about="http://purl.obolibrary.org/obo/GAZ_00237331">
        <obo:RO_0001025 rdf:resource="http://purl.obolibrary.org/obo/GAZ_00015530"/>
        <obo:IAO_0000115>A fourth-level administrative division of Uganda.</obo:IAO_0000115>
        <oboInOwl:hasOBONamespace>GAZ</oboInOwl:hasOBONamespace>
        <oboInOwl:id>GAZ:00237331</oboInOwl:id>
        <rdfs:label>Mpara Sub-county</rdfs:label>
    </owl:NamedIndividual>
    


    <!-- http://purl.obolibrary.org/obo/GAZ_00237332 -->

    <owl:NamedIndividual rdf:about="http://purl.obolibrary.org/obo/GAZ_00237332">
        <obo:RO_0001025 rdf:resource="http://purl.obolibrary.org/obo/GAZ_00015531"/>
        <obo:IAO_0000115>A fourth-level administrative division of Uganda.</obo:IAO_0000115>
        <oboInOwl:hasOBONamespace>GAZ</oboInOwl:hasOBONamespace>
        <oboInOwl:id>GAZ:00237332</oboInOwl:id>
        <rdfs:label>Bufunjo Sub-county</rdfs:label>
    </owl:NamedIndividual>
    


    <!-- http://purl.obolibrary.org/obo/GAZ_00237333 -->

    <owl:NamedIndividual rdf:about="http://purl.obolibrary.org/obo/GAZ_00237333">
        <obo:RO_0001025 rdf:resource="http://purl.obolibrary.org/obo/GAZ_00015531"/>
        <obo:IAO_0000115>A fourth-level administrative division of Uganda.</obo:IAO_0000115>
        <oboInOwl:hasOBONamespace>GAZ</oboInOwl:hasOBONamespace>
        <oboInOwl:id>GAZ:00237333</oboInOwl:id>
        <rdfs:label>Bugaaki Sub-county</rdfs:label>
    </owl:NamedIndividual>
    


    <!-- http://purl.obolibrary.org/obo/GAZ_00237334 -->

    <owl:NamedIndividual rdf:about="http://purl.obolibrary.org/obo/GAZ_00237334">
        <obo:RO_0001025 rdf:resource="http://purl.obolibrary.org/obo/GAZ_00015531"/>
        <obo:IAO_0000115>A fourth-level administrative division of Uganda.</obo:IAO_0000115>
        <oboInOwl:hasOBONamespace>GAZ</oboInOwl:hasOBONamespace>
        <oboInOwl:id>GAZ:00237334</oboInOwl:id>
        <rdfs:label>Butiiti Sub-county</rdfs:label>
    </owl:NamedIndividual>
    


    <!-- http://purl.obolibrary.org/obo/GAZ_00237335 -->

    <owl:NamedIndividual rdf:about="http://purl.obolibrary.org/obo/GAZ_00237335">
        <obo:RO_0001025 rdf:resource="http://purl.obolibrary.org/obo/GAZ_00015531"/>
        <obo:IAO_0000115>A fourth-level administrative division of Uganda.</obo:IAO_0000115>
        <oboInOwl:hasOBONamespace>GAZ</oboInOwl:hasOBONamespace>
        <oboInOwl:id>GAZ:00237335</oboInOwl:id>
        <rdfs:label>Katoke Sub-county</rdfs:label>
    </owl:NamedIndividual>
    


    <!-- http://purl.obolibrary.org/obo/GAZ_00237336 -->

    <owl:NamedIndividual rdf:about="http://purl.obolibrary.org/obo/GAZ_00237336">
        <obo:RO_0001025 rdf:resource="http://purl.obolibrary.org/obo/GAZ_00015531"/>
        <obo:IAO_0000115>A fourth-level administrative division of Uganda.</obo:IAO_0000115>
        <oboInOwl:hasOBONamespace>GAZ</oboInOwl:hasOBONamespace>
        <oboInOwl:id>GAZ:00237336</oboInOwl:id>
        <rdfs:label>Kihuura Sub-county</rdfs:label>
    </owl:NamedIndividual>
    


    <!-- http://purl.obolibrary.org/obo/GAZ_00237337 -->

    <owl:NamedIndividual rdf:about="http://purl.obolibrary.org/obo/GAZ_00237337">
        <obo:RO_0001025 rdf:resource="http://purl.obolibrary.org/obo/GAZ_00015531"/>
        <obo:IAO_0000115>A fourth-level administrative division of Uganda.</obo:IAO_0000115>
        <oboInOwl:hasOBONamespace>GAZ</oboInOwl:hasOBONamespace>
        <oboInOwl:id>GAZ:00237337</oboInOwl:id>
        <rdfs:label>Kyarusozi Sub-county</rdfs:label>
    </owl:NamedIndividual>
    


    <!-- http://purl.obolibrary.org/obo/GAZ_00237338 -->

    <owl:NamedIndividual rdf:about="http://purl.obolibrary.org/obo/GAZ_00237338">
        <obo:RO_0001025 rdf:resource="http://purl.obolibrary.org/obo/GAZ_00015531"/>
        <obo:IAO_0000115>A fourth-level administrative division of Uganda.</obo:IAO_0000115>
        <oboInOwl:hasOBONamespace>GAZ</oboInOwl:hasOBONamespace>
        <oboInOwl:id>GAZ:00237338</oboInOwl:id>
        <rdfs:label>Kyenjojo Town</rdfs:label>
    </owl:NamedIndividual>
    


    <!-- http://purl.obolibrary.org/obo/GAZ_00237339 -->

    <owl:NamedIndividual rdf:about="http://purl.obolibrary.org/obo/GAZ_00237339">
        <obo:RO_0001025 rdf:resource="http://purl.obolibrary.org/obo/GAZ_00015531"/>
        <obo:IAO_0000115>A fourth-level administrative division of Uganda.</obo:IAO_0000115>
        <oboInOwl:hasOBONamespace>GAZ</oboInOwl:hasOBONamespace>
        <oboInOwl:id>GAZ:00237339</oboInOwl:id>
        <rdfs:label>Nyankwanzi Sub-county</rdfs:label>
    </owl:NamedIndividual>
    


    <!-- http://purl.obolibrary.org/obo/GAZ_00237340 -->

    <owl:NamedIndividual rdf:about="http://purl.obolibrary.org/obo/GAZ_00237340">
        <obo:RO_0001025 rdf:resource="http://purl.obolibrary.org/obo/GAZ_00015531"/>
        <obo:IAO_0000115>A fourth-level administrative division of Uganda.</obo:IAO_0000115>
        <oboInOwl:hasOBONamespace>GAZ</oboInOwl:hasOBONamespace>
        <oboInOwl:id>GAZ:00237340</oboInOwl:id>
        <rdfs:label>Nyantungo Sub-county</rdfs:label>
    </owl:NamedIndividual>
    


    <!-- http://purl.obolibrary.org/obo/GAZ_00237341 -->

    <owl:NamedIndividual rdf:about="http://purl.obolibrary.org/obo/GAZ_00237341">
        <obo:RO_0001025 rdf:resource="http://purl.obolibrary.org/obo/GAZ_00076730"/>
        <obo:IAO_0000115>A protected area.</obo:IAO_0000115>
        <oboInOwl:hasOBONamespace>GAZ</oboInOwl:hasOBONamespace>
        <oboInOwl:id>GAZ:00237341</oboInOwl:id>
        <rdfs:label>Bugungu Wildlife Reserve</rdfs:label>
    </owl:NamedIndividual>
    


    <!-- http://purl.obolibrary.org/obo/GAZ_00237342 -->

    <owl:NamedIndividual rdf:about="http://purl.obolibrary.org/obo/GAZ_00237342">
        <obo:RO_0001025 rdf:resource="http://purl.obolibrary.org/obo/GAZ_00076730"/>
        <obo:IAO_0000115>A protected area.</obo:IAO_0000115>
        <oboInOwl:hasOBONamespace>GAZ</oboInOwl:hasOBONamespace>
        <oboInOwl:id>GAZ:00237342</oboInOwl:id>
        <rdfs:label>Karuma Wildlife Reserve</rdfs:label>
    </owl:NamedIndividual>
    


    <!-- http://purl.obolibrary.org/obo/GAZ_00237343 -->

    <owl:NamedIndividual rdf:about="http://purl.obolibrary.org/obo/GAZ_00237343">
        <obo:RO_0001025 rdf:resource="http://purl.obolibrary.org/obo/GAZ_00009915"/>
        <obo:IAO_0000115>A protected area.</obo:IAO_0000115>
        <oboInOwl:hasOBONamespace>GAZ</oboInOwl:hasOBONamespace>
        <oboInOwl:id>GAZ:00237343</oboInOwl:id>
        <rdfs:label>Budongo Forest Reserve</rdfs:label>
    </owl:NamedIndividual>
    


    <!-- http://purl.obolibrary.org/obo/GAZ_00237344 -->

    <owl:NamedIndividual rdf:about="http://purl.obolibrary.org/obo/GAZ_00237344">
        <obo:RO_0001025 rdf:resource="http://purl.obolibrary.org/obo/GAZ_00237343"/>
        <obo:IAO_0000115>A research station.</obo:IAO_0000115>
        <oboInOwl:hasOBONamespace>GAZ</oboInOwl:hasOBONamespace>
        <oboInOwl:id>GAZ:00237344</oboInOwl:id>
        <rdfs:label>Budongo Conservation Field Station</rdfs:label>
    </owl:NamedIndividual>
    


    <!-- http://purl.obolibrary.org/obo/GAZ_00237345 -->

    <owl:NamedIndividual rdf:about="http://purl.obolibrary.org/obo/GAZ_00237345">
        <obo:RO_0001025 rdf:resource="http://purl.obolibrary.org/obo/GAZ_00015527"/>
        <obo:IAO_0000115>A fourth-level administrative division of Uganda.</obo:IAO_0000115>
        <oboInOwl:hasOBONamespace>GAZ</oboInOwl:hasOBONamespace>
        <oboInOwl:id>GAZ:00237345</oboInOwl:id>
        <rdfs:label>Budongo Sub-county</rdfs:label>
    </owl:NamedIndividual>
    


    <!-- http://purl.obolibrary.org/obo/GAZ_00237346 -->

    <owl:NamedIndividual rdf:about="http://purl.obolibrary.org/obo/GAZ_00237346">
        <obo:RO_0001025 rdf:resource="http://purl.obolibrary.org/obo/GAZ_00015527"/>
        <obo:IAO_0000115>A fourth-level administrative division of Uganda.</obo:IAO_0000115>
        <oboInOwl:hasOBONamespace>GAZ</oboInOwl:hasOBONamespace>
        <oboInOwl:id>GAZ:00237346</oboInOwl:id>
        <rdfs:label>Bwijanga Sub-county</rdfs:label>
    </owl:NamedIndividual>
    


    <!-- http://purl.obolibrary.org/obo/GAZ_00237347 -->

    <owl:NamedIndividual rdf:about="http://purl.obolibrary.org/obo/GAZ_00237347">
        <obo:RO_0001025 rdf:resource="http://purl.obolibrary.org/obo/GAZ_00015529"/>
        <obo:IAO_0000115>A fourth-level administrative division of Uganda.</obo:IAO_0000115>
        <oboInOwl:hasOBONamespace>GAZ</oboInOwl:hasOBONamespace>
        <oboInOwl:id>GAZ:00237347</oboInOwl:id>
        <rdfs:label>Karujubu Sub-county</rdfs:label>
    </owl:NamedIndividual>
    


    <!-- http://purl.obolibrary.org/obo/GAZ_00237348 -->

    <owl:NamedIndividual rdf:about="http://purl.obolibrary.org/obo/GAZ_00237348">
        <obo:RO_0001025 rdf:resource="http://purl.obolibrary.org/obo/GAZ_00015529"/>
        <obo:IAO_0000115>A fourth-level administrative division of Uganda.</obo:IAO_0000115>
        <oboInOwl:hasOBONamespace>GAZ</oboInOwl:hasOBONamespace>
        <oboInOwl:id>GAZ:00237348</oboInOwl:id>
        <rdfs:label>Kimengo Sub-county</rdfs:label>
    </owl:NamedIndividual>
    


    <!-- http://purl.obolibrary.org/obo/GAZ_00237349 -->

    <owl:NamedIndividual rdf:about="http://purl.obolibrary.org/obo/GAZ_00237349">
        <obo:RO_0001025 rdf:resource="http://purl.obolibrary.org/obo/GAZ_00015529"/>
        <obo:IAO_0000115>A fourth-level administrative division of Uganda.</obo:IAO_0000115>
        <oboInOwl:hasOBONamespace>GAZ</oboInOwl:hasOBONamespace>
        <oboInOwl:id>GAZ:00237349</oboInOwl:id>
        <rdfs:label>Masindi Town</rdfs:label>
    </owl:NamedIndividual>
    


    <!-- http://purl.obolibrary.org/obo/GAZ_00237350 -->

    <owl:NamedIndividual rdf:about="http://purl.obolibrary.org/obo/GAZ_00237350">
        <obo:RO_0001025 rdf:resource="http://purl.obolibrary.org/obo/GAZ_00015529"/>
        <obo:IAO_0000115>A fourth-level administrative division of Uganda.</obo:IAO_0000115>
        <oboInOwl:hasOBONamespace>GAZ</oboInOwl:hasOBONamespace>
        <oboInOwl:id>GAZ:00237350</oboInOwl:id>
        <rdfs:label>Miirya Sub-county</rdfs:label>
    </owl:NamedIndividual>
    


    <!-- http://purl.obolibrary.org/obo/GAZ_00237351 -->

    <owl:NamedIndividual rdf:about="http://purl.obolibrary.org/obo/GAZ_00237351">
        <obo:RO_0001025 rdf:resource="http://purl.obolibrary.org/obo/GAZ_00015529"/>
        <obo:IAO_0000115>A fourth-level administrative division of Uganda.</obo:IAO_0000115>
        <oboInOwl:hasOBONamespace>GAZ</oboInOwl:hasOBONamespace>
        <oboInOwl:id>GAZ:00237351</oboInOwl:id>
        <rdfs:label>Nyangahya Sub-county</rdfs:label>
    </owl:NamedIndividual>
    


    <!-- http://purl.obolibrary.org/obo/GAZ_00237352 -->

    <owl:NamedIndividual rdf:about="http://purl.obolibrary.org/obo/GAZ_00237352">
        <obo:RO_0001025 rdf:resource="http://purl.obolibrary.org/obo/GAZ_00015529"/>
        <obo:IAO_0000115>A fourth-level administrative division of Uganda.</obo:IAO_0000115>
        <oboInOwl:hasOBONamespace>GAZ</oboInOwl:hasOBONamespace>
        <oboInOwl:id>GAZ:00237352</oboInOwl:id>
        <rdfs:label>Pakanyi Sub-county</rdfs:label>
    </owl:NamedIndividual>
    


    <!-- http://purl.obolibrary.org/obo/GAZ_00237353 -->

    <owl:NamedIndividual rdf:about="http://purl.obolibrary.org/obo/GAZ_00237353">
        <obo:RO_0001025 rdf:resource="http://purl.obolibrary.org/obo/GAZ_00015528"/>
        <obo:IAO_0000115>A fourth-level administrative division of Uganda.</obo:IAO_0000115>
        <oboInOwl:hasOBONamespace>GAZ</oboInOwl:hasOBONamespace>
        <oboInOwl:id>GAZ:00237353</oboInOwl:id>
        <rdfs:label>Kigumba Sub-county</rdfs:label>
    </owl:NamedIndividual>
    


    <!-- http://purl.obolibrary.org/obo/GAZ_00237354 -->

    <owl:NamedIndividual rdf:about="http://purl.obolibrary.org/obo/GAZ_00237354">
        <obo:RO_0001025 rdf:resource="http://purl.obolibrary.org/obo/GAZ_00015528"/>
        <obo:IAO_0000115>A fourth-level administrative division of Uganda.</obo:IAO_0000115>
        <oboInOwl:hasOBONamespace>GAZ</oboInOwl:hasOBONamespace>
        <oboInOwl:id>GAZ:00237354</oboInOwl:id>
        <rdfs:label>Kiryandongo Sub-county</rdfs:label>
    </owl:NamedIndividual>
    


    <!-- http://purl.obolibrary.org/obo/GAZ_00237355 -->

    <owl:NamedIndividual rdf:about="http://purl.obolibrary.org/obo/GAZ_00237355">
        <obo:RO_0001025 rdf:resource="http://purl.obolibrary.org/obo/GAZ_00015528"/>
        <obo:IAO_0000115>A fourth-level administrative division of Uganda.</obo:IAO_0000115>
        <oboInOwl:hasOBONamespace>GAZ</oboInOwl:hasOBONamespace>
        <oboInOwl:id>GAZ:00237355</oboInOwl:id>
        <rdfs:label>Masindi-Port Sub-county</rdfs:label>
    </owl:NamedIndividual>
    


    <!-- http://purl.obolibrary.org/obo/GAZ_00237356 -->

    <owl:NamedIndividual rdf:about="http://purl.obolibrary.org/obo/GAZ_00237356">
        <obo:RO_0001025 rdf:resource="http://purl.obolibrary.org/obo/GAZ_00015528"/>
        <obo:IAO_0000115>A fourth-level administrative division of Uganda.</obo:IAO_0000115>
        <oboInOwl:hasOBONamespace>GAZ</oboInOwl:hasOBONamespace>
        <oboInOwl:id>GAZ:00237356</oboInOwl:id>
        <rdfs:label>Mutunda Sub-county</rdfs:label>
    </owl:NamedIndividual>
    


    <!-- http://purl.obolibrary.org/obo/GAZ_00237357 -->

    <owl:NamedIndividual rdf:about="http://purl.obolibrary.org/obo/GAZ_00237357">
        <obo:RO_0001025 rdf:resource="http://purl.obolibrary.org/obo/GAZ_00015525"/>
        <obo:IAO_0000115>A fourth-level administrative division of Uganda.</obo:IAO_0000115>
        <oboInOwl:hasOBONamespace>GAZ</oboInOwl:hasOBONamespace>
        <oboInOwl:id>GAZ:00237357</oboInOwl:id>
        <rdfs:label>Bubaare Sub-county</rdfs:label>
    </owl:NamedIndividual>
    


    <!-- http://purl.obolibrary.org/obo/GAZ_00237358 -->

    <owl:NamedIndividual rdf:about="http://purl.obolibrary.org/obo/GAZ_00237358">
        <obo:RO_0001025 rdf:resource="http://purl.obolibrary.org/obo/GAZ_00015525"/>
        <obo:IAO_0000115>A fourth-level administrative division of Uganda.</obo:IAO_0000115>
        <oboInOwl:hasOBONamespace>GAZ</oboInOwl:hasOBONamespace>
        <oboInOwl:id>GAZ:00237358</oboInOwl:id>
        <rdfs:label>Bukiro Sub-county</rdfs:label>
    </owl:NamedIndividual>
    


    <!-- http://purl.obolibrary.org/obo/GAZ_00237359 -->

    <owl:NamedIndividual rdf:about="http://purl.obolibrary.org/obo/GAZ_00237359">
        <obo:RO_0001025 rdf:resource="http://purl.obolibrary.org/obo/GAZ_00015525"/>
        <obo:IAO_0000115>A fourth-level administrative division of Uganda.</obo:IAO_0000115>
        <oboInOwl:hasOBONamespace>GAZ</oboInOwl:hasOBONamespace>
        <oboInOwl:id>GAZ:00237359</oboInOwl:id>
        <rdfs:label>Kagongi Sub-county</rdfs:label>
    </owl:NamedIndividual>
    


    <!-- http://purl.obolibrary.org/obo/GAZ_00237360 -->

    <owl:NamedIndividual rdf:about="http://purl.obolibrary.org/obo/GAZ_00237360">
        <obo:RO_0001025 rdf:resource="http://purl.obolibrary.org/obo/GAZ_00015525"/>
        <obo:IAO_0000115>A fourth-level administrative division of Uganda.</obo:IAO_0000115>
        <oboInOwl:hasOBONamespace>GAZ</oboInOwl:hasOBONamespace>
        <oboInOwl:id>GAZ:00237360</oboInOwl:id>
        <rdfs:label>Kakiika Sub-county</rdfs:label>
    </owl:NamedIndividual>
    


    <!-- http://purl.obolibrary.org/obo/GAZ_00237361 -->

    <owl:NamedIndividual rdf:about="http://purl.obolibrary.org/obo/GAZ_00237361">
        <obo:RO_0001025 rdf:resource="http://purl.obolibrary.org/obo/GAZ_00015525"/>
        <obo:IAO_0000115>A fourth-level administrative division of Uganda.</obo:IAO_0000115>
        <oboInOwl:hasOBONamespace>GAZ</oboInOwl:hasOBONamespace>
        <oboInOwl:id>GAZ:00237361</oboInOwl:id>
        <rdfs:label>Kashare Sub-county</rdfs:label>
    </owl:NamedIndividual>
    


    <!-- http://purl.obolibrary.org/obo/GAZ_00237362 -->

    <owl:NamedIndividual rdf:about="http://purl.obolibrary.org/obo/GAZ_00237362">
        <obo:RO_0001025 rdf:resource="http://purl.obolibrary.org/obo/GAZ_00015525"/>
        <obo:IAO_0000115>A fourth-level administrative division of Uganda.</obo:IAO_0000115>
        <oboInOwl:hasOBONamespace>GAZ</oboInOwl:hasOBONamespace>
        <oboInOwl:id>GAZ:00237362</oboInOwl:id>
        <rdfs:label>Rubaya Sub-county</rdfs:label>
    </owl:NamedIndividual>
    


    <!-- http://purl.obolibrary.org/obo/GAZ_00237363 -->

    <owl:NamedIndividual rdf:about="http://purl.obolibrary.org/obo/GAZ_00237363">
        <obo:RO_0001025 rdf:resource="http://purl.obolibrary.org/obo/GAZ_00015525"/>
        <obo:IAO_0000115>A fourth-level administrative division of Uganda.</obo:IAO_0000115>
        <oboInOwl:hasOBONamespace>GAZ</oboInOwl:hasOBONamespace>
        <oboInOwl:id>GAZ:00237363</oboInOwl:id>
        <rdfs:label>Rubindi Sub-county</rdfs:label>
    </owl:NamedIndividual>
    


    <!-- http://purl.obolibrary.org/obo/GAZ_00237364 -->

    <owl:NamedIndividual rdf:about="http://purl.obolibrary.org/obo/GAZ_00237364">
        <obo:RO_0001025 rdf:resource="http://purl.obolibrary.org/obo/GAZ_00015525"/>
        <obo:IAO_0000115>A fourth-level administrative division of Uganda.</obo:IAO_0000115>
        <oboInOwl:hasOBONamespace>GAZ</oboInOwl:hasOBONamespace>
        <oboInOwl:id>GAZ:00237364</oboInOwl:id>
        <rdfs:label>Rwanyamahembe Sub-county</rdfs:label>
    </owl:NamedIndividual>
    


    <!-- http://purl.obolibrary.org/obo/GAZ_00237365 -->

    <owl:NamedIndividual rdf:about="http://purl.obolibrary.org/obo/GAZ_00237365">
        <obo:RO_0001025 rdf:resource="http://purl.obolibrary.org/obo/GAZ_00015526"/>
        <obo:IAO_0000115>A fourth-level administrative division of Uganda.</obo:IAO_0000115>
        <oboInOwl:hasOBONamespace>GAZ</oboInOwl:hasOBONamespace>
        <oboInOwl:id>GAZ:00237365</oboInOwl:id>
        <rdfs:label>Bugamba Sub-county</rdfs:label>
    </owl:NamedIndividual>
    


    <!-- http://purl.obolibrary.org/obo/GAZ_00237366 -->

    <owl:NamedIndividual rdf:about="http://purl.obolibrary.org/obo/GAZ_00237366">
        <obo:RO_0001025 rdf:resource="http://purl.obolibrary.org/obo/GAZ_00015526"/>
        <obo:IAO_0000115>A fourth-level administrative division of Uganda.</obo:IAO_0000115>
        <oboInOwl:hasOBONamespace>GAZ</oboInOwl:hasOBONamespace>
        <oboInOwl:id>GAZ:00237366</oboInOwl:id>
        <rdfs:label>Mwizi Sub-county</rdfs:label>
    </owl:NamedIndividual>
    


    <!-- http://purl.obolibrary.org/obo/GAZ_00237367 -->

    <owl:NamedIndividual rdf:about="http://purl.obolibrary.org/obo/GAZ_00237367">
        <obo:RO_0001025 rdf:resource="http://purl.obolibrary.org/obo/GAZ_00015526"/>
        <obo:IAO_0000115>A fourth-level administrative division of Uganda.</obo:IAO_0000115>
        <oboInOwl:hasOBONamespace>GAZ</oboInOwl:hasOBONamespace>
        <oboInOwl:id>GAZ:00237367</oboInOwl:id>
        <rdfs:label>Ndaija Sub-county</rdfs:label>
    </owl:NamedIndividual>
    


    <!-- http://purl.obolibrary.org/obo/GAZ_00237368 -->

    <owl:NamedIndividual rdf:about="http://purl.obolibrary.org/obo/GAZ_00237368">
        <obo:RO_0001025 rdf:resource="http://purl.obolibrary.org/obo/GAZ_00015526"/>
        <obo:IAO_0000115>A fourth-level administrative division of Uganda.</obo:IAO_0000115>
        <oboInOwl:hasOBONamespace>GAZ</oboInOwl:hasOBONamespace>
        <oboInOwl:id>GAZ:00237368</oboInOwl:id>
        <rdfs:label>Nyakayojo Sub-county</rdfs:label>
    </owl:NamedIndividual>
    


    <!-- http://purl.obolibrary.org/obo/GAZ_00237369 -->

    <owl:NamedIndividual rdf:about="http://purl.obolibrary.org/obo/GAZ_00237369">
        <obo:RO_0001025 rdf:resource="http://purl.obolibrary.org/obo/GAZ_00015526"/>
        <obo:IAO_0000115>A fourth-level administrative division of Uganda.</obo:IAO_0000115>
        <oboInOwl:hasOBONamespace>GAZ</oboInOwl:hasOBONamespace>
        <oboInOwl:id>GAZ:00237369</oboInOwl:id>
        <rdfs:label>Rugando Sub-county</rdfs:label>
    </owl:NamedIndividual>
    


    <!-- http://purl.obolibrary.org/obo/GAZ_00237370 -->

    <owl:NamedIndividual rdf:about="http://purl.obolibrary.org/obo/GAZ_00237370">
        <obo:RO_0001025 rdf:resource="http://purl.obolibrary.org/obo/GAZ_00009918"/>
        <obo:IAO_0000115>A fourth-level administrative division of Uganda.</obo:IAO_0000115>
        <oboInOwl:hasOBONamespace>GAZ</oboInOwl:hasOBONamespace>
        <oboInOwl:id>GAZ:00237370</oboInOwl:id>
        <rdfs:label>Kakoba Division</rdfs:label>
    </owl:NamedIndividual>
    


    <!-- http://purl.obolibrary.org/obo/GAZ_00237371 -->

    <owl:NamedIndividual rdf:about="http://purl.obolibrary.org/obo/GAZ_00237371">
        <obo:RO_0001025 rdf:resource="http://purl.obolibrary.org/obo/GAZ_00009918"/>
        <obo:IAO_0000115>A fourth-level administrative division of Uganda.</obo:IAO_0000115>
        <oboInOwl:hasOBONamespace>GAZ</oboInOwl:hasOBONamespace>
        <oboInOwl:id>GAZ:00237371</oboInOwl:id>
        <rdfs:label>Kamukuzi Division</rdfs:label>
    </owl:NamedIndividual>
    


    <!-- http://purl.obolibrary.org/obo/GAZ_00237372 -->

    <owl:NamedIndividual rdf:about="http://purl.obolibrary.org/obo/GAZ_00237372">
        <obo:RO_0001025 rdf:resource="http://purl.obolibrary.org/obo/GAZ_00009918"/>
        <obo:IAO_0000115>A fourth-level administrative division of Uganda.</obo:IAO_0000115>
        <oboInOwl:hasOBONamespace>GAZ</oboInOwl:hasOBONamespace>
        <oboInOwl:id>GAZ:00237372</oboInOwl:id>
        <rdfs:label>Nyamitanga Division</rdfs:label>
    </owl:NamedIndividual>
    


    <!-- http://purl.obolibrary.org/obo/GAZ_00237373 -->

    <owl:NamedIndividual rdf:about="http://purl.obolibrary.org/obo/GAZ_00237373">
        <obo:RO_0001025 rdf:resource="http://purl.obolibrary.org/obo/GAZ_00015523"/>
        <obo:IAO_0000115>A fourth-level administrative division of Uganda.</obo:IAO_0000115>
        <oboInOwl:hasOBONamespace>GAZ</oboInOwl:hasOBONamespace>
        <oboInOwl:id>GAZ:00237373</oboInOwl:id>
        <rdfs:label>Bwongyera Sub-county</rdfs:label>
    </owl:NamedIndividual>
    


    <!-- http://purl.obolibrary.org/obo/GAZ_00237374 -->

    <owl:NamedIndividual rdf:about="http://purl.obolibrary.org/obo/GAZ_00237374">
        <obo:RO_0001025 rdf:resource="http://purl.obolibrary.org/obo/GAZ_00015523"/>
        <obo:IAO_0000115>A fourth-level administrative division of Uganda.</obo:IAO_0000115>
        <oboInOwl:hasOBONamespace>GAZ</oboInOwl:hasOBONamespace>
        <oboInOwl:id>GAZ:00237374</oboInOwl:id>
        <rdfs:label>Ihunga Sub-county</rdfs:label>
    </owl:NamedIndividual>
    


    <!-- http://purl.obolibrary.org/obo/GAZ_00237375 -->

    <owl:NamedIndividual rdf:about="http://purl.obolibrary.org/obo/GAZ_00237375">
        <obo:RO_0001025 rdf:resource="http://purl.obolibrary.org/obo/GAZ_00015523"/>
        <obo:IAO_0000115>A fourth-level administrative division of Uganda.</obo:IAO_0000115>
        <oboInOwl:hasOBONamespace>GAZ</oboInOwl:hasOBONamespace>
        <oboInOwl:id>GAZ:00237375</oboInOwl:id>
        <rdfs:label>Kibatsi Sub-county</rdfs:label>
    </owl:NamedIndividual>
    


    <!-- http://purl.obolibrary.org/obo/GAZ_00237376 -->

    <owl:NamedIndividual rdf:about="http://purl.obolibrary.org/obo/GAZ_00237376">
        <obo:RO_0001025 rdf:resource="http://purl.obolibrary.org/obo/GAZ_00015523"/>
        <obo:IAO_0000115>A fourth-level administrative division of Uganda.</obo:IAO_0000115>
        <oboInOwl:hasOBONamespace>GAZ</oboInOwl:hasOBONamespace>
        <oboInOwl:id>GAZ:00237376</oboInOwl:id>
        <rdfs:label>Nyabihoko Sub-county</rdfs:label>
    </owl:NamedIndividual>
    


    <!-- http://purl.obolibrary.org/obo/GAZ_00237377 -->

    <owl:NamedIndividual rdf:about="http://purl.obolibrary.org/obo/GAZ_00237377">
        <obo:RO_0001025 rdf:resource="http://purl.obolibrary.org/obo/GAZ_00015522"/>
        <obo:IAO_0000115>A fourth-level administrative division of Uganda.</obo:IAO_0000115>
        <oboInOwl:hasOBONamespace>GAZ</oboInOwl:hasOBONamespace>
        <oboInOwl:id>GAZ:00237377</oboInOwl:id>
        <rdfs:label>Itojo Sub-county</rdfs:label>
    </owl:NamedIndividual>
    


    <!-- http://purl.obolibrary.org/obo/GAZ_00237378 -->

    <owl:NamedIndividual rdf:about="http://purl.obolibrary.org/obo/GAZ_00237378">
        <obo:RO_0001025 rdf:resource="http://purl.obolibrary.org/obo/GAZ_00015522"/>
        <obo:IAO_0000115>A fourth-level administrative division of Uganda.</obo:IAO_0000115>
        <oboInOwl:hasOBONamespace>GAZ</oboInOwl:hasOBONamespace>
        <oboInOwl:id>GAZ:00237378</oboInOwl:id>
        <rdfs:label>Ntugamo Sub-county</rdfs:label>
    </owl:NamedIndividual>
    


    <!-- http://purl.obolibrary.org/obo/GAZ_00237379 -->

    <owl:NamedIndividual rdf:about="http://purl.obolibrary.org/obo/GAZ_00237379">
        <obo:RO_0001025 rdf:resource="http://purl.obolibrary.org/obo/GAZ_00015522"/>
        <obo:IAO_0000115>A fourth-level administrative division of Uganda.</obo:IAO_0000115>
        <oboInOwl:hasOBONamespace>GAZ</oboInOwl:hasOBONamespace>
        <oboInOwl:id>GAZ:00237379</oboInOwl:id>
        <rdfs:label>Ntungamo Town</rdfs:label>
    </owl:NamedIndividual>
    


    <!-- http://purl.obolibrary.org/obo/GAZ_00237380 -->

    <owl:NamedIndividual rdf:about="http://purl.obolibrary.org/obo/GAZ_00237380">
        <obo:RO_0001025 rdf:resource="http://purl.obolibrary.org/obo/GAZ_00015522"/>
        <obo:IAO_0000115>A fourth-level administrative division of Uganda.</obo:IAO_0000115>
        <oboInOwl:hasOBONamespace>GAZ</oboInOwl:hasOBONamespace>
        <oboInOwl:id>GAZ:00237380</oboInOwl:id>
        <rdfs:label>Nyakyera Sub-county</rdfs:label>
    </owl:NamedIndividual>
    


    <!-- http://purl.obolibrary.org/obo/GAZ_00237381 -->

    <owl:NamedIndividual rdf:about="http://purl.obolibrary.org/obo/GAZ_00237381">
        <obo:RO_0001025 rdf:resource="http://purl.obolibrary.org/obo/GAZ_00015522"/>
        <obo:IAO_0000115>A fourth-level administrative division of Uganda.</obo:IAO_0000115>
        <oboInOwl:hasOBONamespace>GAZ</oboInOwl:hasOBONamespace>
        <oboInOwl:id>GAZ:00237381</oboInOwl:id>
        <rdfs:label>Ruhaama Sub-county</rdfs:label>
    </owl:NamedIndividual>
    


    <!-- http://purl.obolibrary.org/obo/GAZ_00237382 -->

    <owl:NamedIndividual rdf:about="http://purl.obolibrary.org/obo/GAZ_00237382">
        <obo:RO_0001025 rdf:resource="http://purl.obolibrary.org/obo/GAZ_00015522"/>
        <obo:IAO_0000115>A fourth-level administrative division of Uganda.</obo:IAO_0000115>
        <oboInOwl:hasOBONamespace>GAZ</oboInOwl:hasOBONamespace>
        <oboInOwl:id>GAZ:00237382</oboInOwl:id>
        <rdfs:label>Rukoni Sub-county</rdfs:label>
    </owl:NamedIndividual>
    


    <!-- http://purl.obolibrary.org/obo/GAZ_00237383 -->

    <owl:NamedIndividual rdf:about="http://purl.obolibrary.org/obo/GAZ_00237383">
        <obo:RO_0001025 rdf:resource="http://purl.obolibrary.org/obo/GAZ_00015522"/>
        <obo:IAO_0000115>A fourth-level administrative division of Uganda.</obo:IAO_0000115>
        <oboInOwl:hasOBONamespace>GAZ</oboInOwl:hasOBONamespace>
        <oboInOwl:id>GAZ:00237383</oboInOwl:id>
        <rdfs:label>Rweikiniro Sub-county</rdfs:label>
    </owl:NamedIndividual>
    


    <!-- http://purl.obolibrary.org/obo/GAZ_00237384 -->

    <owl:NamedIndividual rdf:about="http://purl.obolibrary.org/obo/GAZ_00237384">
        <obo:RO_0001025 rdf:resource="http://purl.obolibrary.org/obo/GAZ_00015524"/>
        <obo:IAO_0000115>A fourth-level administrative division of Uganda.</obo:IAO_0000115>
        <oboInOwl:hasOBONamespace>GAZ</oboInOwl:hasOBONamespace>
        <oboInOwl:id>GAZ:00237384</oboInOwl:id>
        <rdfs:label>Kayonza Sub-county</rdfs:label>
    </owl:NamedIndividual>
    


    <!-- http://purl.obolibrary.org/obo/GAZ_00237385 -->

    <owl:NamedIndividual rdf:about="http://purl.obolibrary.org/obo/GAZ_00237385">
        <obo:RO_0001025 rdf:resource="http://purl.obolibrary.org/obo/GAZ_00015524"/>
        <obo:IAO_0000115>A fourth-level administrative division of Uganda.</obo:IAO_0000115>
        <oboInOwl:hasOBONamespace>GAZ</oboInOwl:hasOBONamespace>
        <oboInOwl:id>GAZ:00237385</oboInOwl:id>
        <rdfs:label>Ngoma Sub-county</rdfs:label>
    </owl:NamedIndividual>
    


    <!-- http://purl.obolibrary.org/obo/GAZ_00237386 -->

    <owl:NamedIndividual rdf:about="http://purl.obolibrary.org/obo/GAZ_00237386">
        <obo:RO_0001025 rdf:resource="http://purl.obolibrary.org/obo/GAZ_00015524"/>
        <obo:IAO_0000115>A fourth-level administrative division of Uganda.</obo:IAO_0000115>
        <oboInOwl:hasOBONamespace>GAZ</oboInOwl:hasOBONamespace>
        <oboInOwl:id>GAZ:00237386</oboInOwl:id>
        <rdfs:label>Rubaare Sub-county</rdfs:label>
    </owl:NamedIndividual>
    


    <!-- http://purl.obolibrary.org/obo/GAZ_00237387 -->

    <owl:NamedIndividual rdf:about="http://purl.obolibrary.org/obo/GAZ_00237387">
        <obo:RO_0001025 rdf:resource="http://purl.obolibrary.org/obo/GAZ_00015524"/>
        <obo:IAO_0000115>A fourth-level administrative division of Uganda.</obo:IAO_0000115>
        <oboInOwl:hasOBONamespace>GAZ</oboInOwl:hasOBONamespace>
        <oboInOwl:id>GAZ:00237387</oboInOwl:id>
        <rdfs:label>Rugarama Sub-county</rdfs:label>
    </owl:NamedIndividual>
    


    <!-- http://purl.obolibrary.org/obo/GAZ_00237388 -->

    <owl:NamedIndividual rdf:about="http://purl.obolibrary.org/obo/GAZ_00237388">
        <obo:RO_0001025 rdf:resource="http://purl.obolibrary.org/obo/GAZ_00015520"/>
        <obo:IAO_0000115>A fourth-level administrative division of Uganda.</obo:IAO_0000115>
        <oboInOwl:hasOBONamespace>GAZ</oboInOwl:hasOBONamespace>
        <oboInOwl:id>GAZ:00237388</oboInOwl:id>
        <rdfs:label>Buyanja Sub-county</rdfs:label>
    </owl:NamedIndividual>
    


    <!-- http://purl.obolibrary.org/obo/GAZ_00237389 -->

    <owl:NamedIndividual rdf:about="http://purl.obolibrary.org/obo/GAZ_00237389">
        <obo:RO_0001025 rdf:resource="http://purl.obolibrary.org/obo/GAZ_00015520"/>
        <obo:IAO_0000115>A fourth-level administrative division of Uganda.</obo:IAO_0000115>
        <oboInOwl:hasOBONamespace>GAZ</oboInOwl:hasOBONamespace>
        <oboInOwl:id>GAZ:00237389</oboInOwl:id>
        <rdfs:label>Kebisoni Sub-county</rdfs:label>
    </owl:NamedIndividual>
    


    <!-- http://purl.obolibrary.org/obo/GAZ_00237390 -->

    <owl:NamedIndividual rdf:about="http://purl.obolibrary.org/obo/GAZ_00237390">
        <obo:RO_0001025 rdf:resource="http://purl.obolibrary.org/obo/GAZ_00015520"/>
        <obo:IAO_0000115>A fourth-level administrative division of Uganda.</obo:IAO_0000115>
        <oboInOwl:hasOBONamespace>GAZ</oboInOwl:hasOBONamespace>
        <oboInOwl:id>GAZ:00237390</oboInOwl:id>
        <rdfs:label>Nyakishenyi Sub-county</rdfs:label>
    </owl:NamedIndividual>
    


    <!-- http://purl.obolibrary.org/obo/GAZ_00237391 -->

    <owl:NamedIndividual rdf:about="http://purl.obolibrary.org/obo/GAZ_00237391">
        <obo:RO_0001025 rdf:resource="http://purl.obolibrary.org/obo/GAZ_00015520"/>
        <obo:IAO_0000115>A fourth-level administrative division of Uganda.</obo:IAO_0000115>
        <oboInOwl:hasOBONamespace>GAZ</oboInOwl:hasOBONamespace>
        <oboInOwl:id>GAZ:00237391</oboInOwl:id>
        <rdfs:label>Nyarushanje Sub-county</rdfs:label>
    </owl:NamedIndividual>
    


    <!-- http://purl.obolibrary.org/obo/GAZ_00237392 -->

    <owl:NamedIndividual rdf:about="http://purl.obolibrary.org/obo/GAZ_00237392">
        <obo:RO_0001025 rdf:resource="http://purl.obolibrary.org/obo/GAZ_00015521"/>
        <obo:IAO_0000115>A fourth-level administrative division of Uganda.</obo:IAO_0000115>
        <oboInOwl:hasOBONamespace>GAZ</oboInOwl:hasOBONamespace>
        <oboInOwl:id>GAZ:00237392</oboInOwl:id>
        <rdfs:label>Bugangari Sub-county</rdfs:label>
    </owl:NamedIndividual>
    


    <!-- http://purl.obolibrary.org/obo/GAZ_00237393 -->

    <owl:NamedIndividual rdf:about="http://purl.obolibrary.org/obo/GAZ_00237393">
        <obo:RO_0001025 rdf:resource="http://purl.obolibrary.org/obo/GAZ_00015521"/>
        <obo:IAO_0000115>A fourth-level administrative division of Uganda.</obo:IAO_0000115>
        <oboInOwl:hasOBONamespace>GAZ</oboInOwl:hasOBONamespace>
        <oboInOwl:id>GAZ:00237393</oboInOwl:id>
        <rdfs:label>Buhunga Sub-county</rdfs:label>
    </owl:NamedIndividual>
    


    <!-- http://purl.obolibrary.org/obo/GAZ_00237394 -->

    <owl:NamedIndividual rdf:about="http://purl.obolibrary.org/obo/GAZ_00237394">
        <obo:RO_0001025 rdf:resource="http://purl.obolibrary.org/obo/GAZ_00015521"/>
        <obo:IAO_0000115>A fourth-level administrative division of Uganda.</obo:IAO_0000115>
        <oboInOwl:hasOBONamespace>GAZ</oboInOwl:hasOBONamespace>
        <oboInOwl:id>GAZ:00237394</oboInOwl:id>
        <rdfs:label>Bwambara Sub-county</rdfs:label>
    </owl:NamedIndividual>
    


    <!-- http://purl.obolibrary.org/obo/GAZ_00237395 -->

    <owl:NamedIndividual rdf:about="http://purl.obolibrary.org/obo/GAZ_00237395">
        <obo:RO_0001025 rdf:resource="http://purl.obolibrary.org/obo/GAZ_00015521"/>
        <obo:IAO_0000115>A fourth-level administrative division of Uganda.</obo:IAO_0000115>
        <oboInOwl:hasOBONamespace>GAZ</oboInOwl:hasOBONamespace>
        <oboInOwl:id>GAZ:00237395</oboInOwl:id>
        <rdfs:label>Kagunga Sub-county</rdfs:label>
    </owl:NamedIndividual>
    


    <!-- http://purl.obolibrary.org/obo/GAZ_00237396 -->

    <owl:NamedIndividual rdf:about="http://purl.obolibrary.org/obo/GAZ_00237396">
        <obo:RO_0001025 rdf:resource="http://purl.obolibrary.org/obo/GAZ_00015521"/>
        <obo:IAO_0000115>A fourth-level administrative division of Uganda.</obo:IAO_0000115>
        <oboInOwl:hasOBONamespace>GAZ</oboInOwl:hasOBONamespace>
        <oboInOwl:id>GAZ:00237396</oboInOwl:id>
        <rdfs:label>Nyakagyeme Sub-county</rdfs:label>
    </owl:NamedIndividual>
    


    <!-- http://purl.obolibrary.org/obo/GAZ_00237397 -->

    <owl:NamedIndividual rdf:about="http://purl.obolibrary.org/obo/GAZ_00237397">
        <obo:RO_0001025 rdf:resource="http://purl.obolibrary.org/obo/GAZ_00015521"/>
        <obo:IAO_0000115>A fourth-level administrative division of Uganda.</obo:IAO_0000115>
        <oboInOwl:hasOBONamespace>GAZ</oboInOwl:hasOBONamespace>
        <oboInOwl:id>GAZ:00237397</oboInOwl:id>
        <rdfs:label>Ruhinda Sub-county</rdfs:label>
    </owl:NamedIndividual>
    


    <!-- http://purl.obolibrary.org/obo/GAZ_00237398 -->

    <owl:NamedIndividual rdf:about="http://purl.obolibrary.org/obo/GAZ_00237398">
        <obo:RO_0001025 rdf:resource="http://purl.obolibrary.org/obo/GAZ_00015521"/>
        <obo:IAO_0000115>A fourth-level administrative division of Uganda.</obo:IAO_0000115>
        <oboInOwl:hasOBONamespace>GAZ</oboInOwl:hasOBONamespace>
        <oboInOwl:id>GAZ:00237398</oboInOwl:id>
        <rdfs:label>Rukungiri Town</rdfs:label>
    </owl:NamedIndividual>
    


    <!-- http://purl.obolibrary.org/obo/GAZ_00237399 -->

    <owl:NamedIndividual rdf:about="http://purl.obolibrary.org/obo/GAZ_00237399">
        <obo:RO_0001025 rdf:resource="http://purl.obolibrary.org/obo/GAZ_00237394"/>
        <obo:IAO_0000115>Hot springs.</obo:IAO_0000115>
        <oboInOwl:hasOBONamespace>GAZ</oboInOwl:hasOBONamespace>
        <oboInOwl:id>GAZ:00237399</oboInOwl:id>
        <rdfs:label>Ilimbo Hot Springs</rdfs:label>
    </owl:NamedIndividual>
    


    <!-- http://purl.obolibrary.org/obo/GAZ_00237400 -->

    <owl:NamedIndividual rdf:about="http://purl.obolibrary.org/obo/GAZ_00237400">
        <obo:RO_0001025 rdf:resource="http://purl.obolibrary.org/obo/GAZ_00237389"/>
        <obo:IAO_0000115>Hot springs.</obo:IAO_0000115>
        <oboInOwl:hasOBONamespace>GAZ</oboInOwl:hasOBONamespace>
        <oboInOwl:id>GAZ:00237400</oboInOwl:id>
        <rdfs:label>Minera Hot Springs</rdfs:label>
    </owl:NamedIndividual>
    


    <!-- http://purl.obolibrary.org/obo/GAZ_00237401 -->

    <owl:NamedIndividual rdf:about="http://purl.obolibrary.org/obo/GAZ_00237401">
        <obo:RO_0001025 rdf:resource="http://purl.obolibrary.org/obo/GAZ_00053525"/>
        <obo:IAO_0000115>A crater lake.</obo:IAO_0000115>
        <oboInOwl:hasOBONamespace>GAZ</oboInOwl:hasOBONamespace>
        <oboInOwl:id>GAZ:00237401</oboInOwl:id>
        <rdfs:label>Lake Katunga</rdfs:label>
    </owl:NamedIndividual>
    


    <!-- http://purl.obolibrary.org/obo/GAZ_00237402 -->

    <owl:NamedIndividual rdf:about="http://purl.obolibrary.org/obo/GAZ_00237402">
        <obo:RO_0001025 rdf:resource="http://purl.obolibrary.org/obo/GAZ_00053522"/>
        <obo:RO_0001025 rdf:resource="http://purl.obolibrary.org/obo/GAZ_00076731"/>
        <obo:IAO_0000115>A crater lake.</obo:IAO_0000115>
        <oboInOwl:hasOBONamespace>GAZ</oboInOwl:hasOBONamespace>
        <oboInOwl:id>GAZ:00237402</oboInOwl:id>
        <rdfs:label>Lake Kikorongo</rdfs:label>
    </owl:NamedIndividual>
    


    <!-- http://purl.obolibrary.org/obo/GAZ_00237412 -->

    <owl:NamedIndividual rdf:about="http://purl.obolibrary.org/obo/GAZ_00237412">
        <obo:RO_0001025 rdf:resource="http://purl.obolibrary.org/obo/GAZ_00005376"/>
        <obo:IAO_0000115>A river of eastern Uganda in eastern Africa. It flows in a southern and south-westerly direction and eventually via the Okere River reaches Lake Kyoga.</obo:IAO_0000115>
        <oboInOwl:hasOBONamespace>GAZ</oboInOwl:hasOBONamespace>
        <oboInOwl:id>GAZ:00237412</oboInOwl:id>
        <rdfs:label>Okot River</rdfs:label>
    </owl:NamedIndividual>
    


    <!-- http://purl.obolibrary.org/obo/GAZ_00237449 -->

    <owl:NamedIndividual rdf:about="http://purl.obolibrary.org/obo/GAZ_00237449">
        <obo:IAO_0000115>A river.</obo:IAO_0000115>
        <oboInOwl:hasOBONamespace>GAZ</oboInOwl:hasOBONamespace>
        <oboInOwl:id>GAZ:00237449</oboInOwl:id>
        <rdfs:label>Lufubu River</rdfs:label>
    </owl:NamedIndividual>
    


    <!-- http://purl.obolibrary.org/obo/GAZ_00240890 -->

    <owl:NamedIndividual rdf:about="http://purl.obolibrary.org/obo/GAZ_00240890">
        <obo:RO_0001025 rdf:resource="http://purl.obolibrary.org/obo/GAZ_00008558"/>
        <obo:IAO_0000115>An island.</obo:IAO_0000115>
        <oboInOwl:hasOBONamespace>GAZ</oboInOwl:hasOBONamespace>
        <oboInOwl:id>GAZ:00240890</oboInOwl:id>
        <rdfs:label>Ile Wahu</rdfs:label>
    </owl:NamedIndividual>
    


    <!-- http://purl.obolibrary.org/obo/GAZ_00240891 -->

    <owl:NamedIndividual rdf:about="http://purl.obolibrary.org/obo/GAZ_00240891">
        <obo:RO_0001025 rdf:resource="http://purl.obolibrary.org/obo/GAZ_00008558"/>
        <obo:IAO_0000115>An island.</obo:IAO_0000115>
        <oboInOwl:hasOBONamespace>GAZ</oboInOwl:hasOBONamespace>
        <oboInOwl:id>GAZ:00240891</oboInOwl:id>
        <rdfs:label>Ile Bugarura</rdfs:label>
    </owl:NamedIndividual>
    


    <!-- http://purl.obolibrary.org/obo/GAZ_00240892 -->

    <owl:NamedIndividual rdf:about="http://purl.obolibrary.org/obo/GAZ_00240892">
        <obo:RO_0001025 rdf:resource="http://purl.obolibrary.org/obo/GAZ_00008558"/>
        <obo:IAO_0000115>An island.</obo:IAO_0000115>
        <oboInOwl:hasOBONamespace>GAZ</oboInOwl:hasOBONamespace>
        <oboInOwl:id>GAZ:00240892</oboInOwl:id>
        <rdfs:label>Ile Gombe</rdfs:label>
    </owl:NamedIndividual>
    


    <!-- http://purl.obolibrary.org/obo/GAZ_00247089 -->

    <owl:NamedIndividual rdf:about="http://purl.obolibrary.org/obo/GAZ_00247089">
        <obo:IAO_0000115>A river. A tributary of the Ruvyironza River.</obo:IAO_0000115>
        <oboInOwl:hasOBONamespace>GAZ</oboInOwl:hasOBONamespace>
        <oboInOwl:id>GAZ:00247089</oboInOwl:id>
        <rdfs:label>Karuzi River</rdfs:label>
    </owl:NamedIndividual>
    


    <!-- http://purl.obolibrary.org/obo/GAZ_00247090 -->

    <owl:NamedIndividual rdf:about="http://purl.obolibrary.org/obo/GAZ_00247090">
        <obo:IAO_0000115>A river. It rises in the far east of Burundi, close to the Tanzanian border, and flows southwestwards, anti-parallel with the Rurubu for 48 km, before turning abruptly northwards to a confluence with the Rurubu.</obo:IAO_0000115>
        <oboInOwl:hasOBONamespace>GAZ</oboInOwl:hasOBONamespace>
        <oboInOwl:id>GAZ:00247090</oboInOwl:id>
        <rdfs:label>Kayongozi River</rdfs:label>
    </owl:NamedIndividual>
    


    <!-- http://purl.obolibrary.org/obo/GAZ_00247094 -->

    <owl:NamedIndividual rdf:about="http://purl.obolibrary.org/obo/GAZ_00247094">
        <obo:IAO_0000115>A river that flows into Lake Tanganyika in the south of Burundi.</obo:IAO_0000115>
        <oboInOwl:hasOBONamespace>GAZ</oboInOwl:hasOBONamespace>
        <oboInOwl:id>GAZ:00247094</oboInOwl:id>
        <rdfs:label>Mugwezi River</rdfs:label>
    </owl:NamedIndividual>
    


    <!-- http://purl.obolibrary.org/obo/GAZ_00247095 -->

    <owl:NamedIndividual rdf:about="http://purl.obolibrary.org/obo/GAZ_00247095">
        <obo:IAO_0000115>A river that flows into Lake Tanganyika in the south of Burundi.</obo:IAO_0000115>
        <oboInOwl:hasOBONamespace>GAZ</oboInOwl:hasOBONamespace>
        <oboInOwl:id>GAZ:00247095</oboInOwl:id>
        <rdfs:label>Luaba River</rdfs:label>
    </owl:NamedIndividual>
    


    <!-- http://purl.obolibrary.org/obo/GAZ_00248126 -->

    <owl:NamedIndividual rdf:about="http://purl.obolibrary.org/obo/GAZ_00248126">
        <rdf:type rdf:resource="http://purl.obolibrary.org/obo/ENVO_00000309"/>
        <obo:RO_0001025 rdf:resource="http://purl.obolibrary.org/obo/GAZ_00000007"/>
        <obo:IAO_0000115>A pan.</obo:IAO_0000115>
        <oboInOwl:hasOBONamespace>GAZ</oboInOwl:hasOBONamespace>
        <oboInOwl:id>GAZ:00248126</oboInOwl:id>
        <rdfs:label>Ch&apos;ew Bahir</rdfs:label>
    </owl:NamedIndividual>
    


    <!-- http://purl.obolibrary.org/obo/GAZ_00248136 -->

    <owl:NamedIndividual rdf:about="http://purl.obolibrary.org/obo/GAZ_00248136">
        <obo:RO_0001025 rdf:resource="http://purl.obolibrary.org/obo/GAZ_00051205"/>
        <obo:IAO_0000115>A saline lake.</obo:IAO_0000115>
        <oboInOwl:hasOBONamespace>GAZ</oboInOwl:hasOBONamespace>
        <oboInOwl:id>GAZ:00248136</oboInOwl:id>
        <rdfs:label>Lake Asale</rdfs:label>
    </owl:NamedIndividual>
    


    <!-- http://purl.obolibrary.org/obo/GAZ_00251586 -->

    <owl:NamedIndividual rdf:about="http://purl.obolibrary.org/obo/GAZ_00251586">
        <obo:IAO_0000115>A river that rises in the hills southwest of Irbid city and drains west into the Jordan Valley, entering the Jordan River about 20 km south of Lake Tiberias.</obo:IAO_0000115>
        <oboInOwl:hasOBONamespace>GAZ</oboInOwl:hasOBONamespace>
        <oboInOwl:id>GAZ:00251586</oboInOwl:id>
        <rdfs:label>Wadi Ziglab</rdfs:label>
    </owl:NamedIndividual>
    


    <!-- http://purl.obolibrary.org/obo/GAZ_00251587 -->

    <owl:NamedIndividual rdf:about="http://purl.obolibrary.org/obo/GAZ_00251587">
        <obo:IAO_0000115>A dam. Located about 15 km south-southwest of Ajlun.</obo:IAO_0000115>
        <oboInOwl:hasOBONamespace>GAZ</oboInOwl:hasOBONamespace>
        <oboInOwl:id>GAZ:00251587</oboInOwl:id>
        <rdfs:label>KingTalal Dam</rdfs:label>
    </owl:NamedIndividual>
    


    <!-- http://purl.obolibrary.org/obo/GAZ_00251592 -->

    <owl:NamedIndividual rdf:about="http://purl.obolibrary.org/obo/GAZ_00251592">
        <obo:IAO_0000115>A dam.</obo:IAO_0000115>
        <oboInOwl:hasOBONamespace>GAZ</oboInOwl:hasOBONamespace>
        <oboInOwl:id>GAZ:00251592</oboInOwl:id>
        <rdfs:label>Kafrein Dam</rdfs:label>
    </owl:NamedIndividual>
    


    <!-- http://purl.obolibrary.org/obo/GAZ_00251593 -->

    <owl:NamedIndividual rdf:about="http://purl.obolibrary.org/obo/GAZ_00251593">
        <obo:IAO_0000115>A dam.</obo:IAO_0000115>
        <oboInOwl:hasOBONamespace>GAZ</oboInOwl:hasOBONamespace>
        <oboInOwl:id>GAZ:00251593</oboInOwl:id>
        <rdfs:label>Shu&apos;eib Dam</rdfs:label>
    </owl:NamedIndividual>
    


    <!-- http://purl.obolibrary.org/obo/GAZ_00251594 -->

    <owl:NamedIndividual rdf:about="http://purl.obolibrary.org/obo/GAZ_00251594">
        <obo:RO_0001025 rdf:resource="http://purl.obolibrary.org/obo/GAZ_00044915"/>
        <obo:IAO_0000115>A saline lake.</obo:IAO_0000115>
        <oboInOwl:hasOBONamespace>GAZ</oboInOwl:hasOBONamespace>
        <oboInOwl:id>GAZ:00251594</oboInOwl:id>
        <rdfs:label>Kibed Pool</rdfs:label>
    </owl:NamedIndividual>
    


    <!-- http://purl.obolibrary.org/obo/GAZ_00251595 -->

    <owl:NamedIndividual rdf:about="http://purl.obolibrary.org/obo/GAZ_00251595">
        <obo:IAO_0000115>A wadi. It enters Wadi Mujib from the north only a few km from the shores of the Dead Sea.</obo:IAO_0000115>
        <oboInOwl:hasOBONamespace>GAZ</oboInOwl:hasOBONamespace>
        <oboInOwl:id>GAZ:00251595</oboInOwl:id>
        <rdfs:label>Wadi Hidan</rdfs:label>
    </owl:NamedIndividual>
    


    <!-- http://purl.obolibrary.org/obo/GAZ_00251642 -->

    <owl:NamedIndividual rdf:about="http://purl.obolibrary.org/obo/GAZ_00251642">
        <obo:RO_0001025 rdf:resource="http://purl.obolibrary.org/obo/GAZ_00041537"/>
        <obo:IAO_0000115>A part of Lake Naivasha. It becomes a discrete, but contiguous, basin at low water.</obo:IAO_0000115>
        <oboInOwl:hasOBONamespace>GAZ</oboInOwl:hasOBONamespace>
        <oboInOwl:id>GAZ:00251642</oboInOwl:id>
        <rdfs:label>Lake Oloidien</rdfs:label>
    </owl:NamedIndividual>
    


    <!-- http://purl.obolibrary.org/obo/GAZ_00251652 -->

    <owl:NamedIndividual rdf:about="http://purl.obolibrary.org/obo/GAZ_00251652">
        <obo:RO_0001025 rdf:resource="http://purl.obolibrary.org/obo/GAZ_00000007"/>
        <obo:IAO_0000115>A lake. It is situated on the Nyandarua Plateau at the foot of the Aberdare Mountains.</obo:IAO_0000115>
        <oboInOwl:hasOBONamespace>GAZ</oboInOwl:hasOBONamespace>
        <oboInOwl:id>GAZ:00251652</oboInOwl:id>
        <rdfs:label>Lake Ilpolosat</rdfs:label>
    </owl:NamedIndividual>
    


    <!-- http://purl.obolibrary.org/obo/GAZ_00251653 -->

    <owl:NamedIndividual rdf:about="http://purl.obolibrary.org/obo/GAZ_00251653">
        <obo:IAO_0000115>A river.</obo:IAO_0000115>
        <oboInOwl:hasOBONamespace>GAZ</oboInOwl:hasOBONamespace>
        <oboInOwl:id>GAZ:00251653</oboInOwl:id>
        <rdfs:label>Malewa River</rdfs:label>
    </owl:NamedIndividual>
    


    <!-- http://purl.obolibrary.org/obo/GAZ_00251816 -->

    <owl:NamedIndividual rdf:about="http://purl.obolibrary.org/obo/GAZ_00251816">
        <obo:RO_0001025 rdf:resource="http://purl.obolibrary.org/obo/GAZ_00044906"/>
        <obo:IAO_0000115>A wetland. Located in the western Beka&apos;a Valley south of the main Beirut to Damascus highway, 10 km south-southwest of Qabb Elias town and about 35 km southeast of Beirut.</obo:IAO_0000115>
        <oboInOwl:hasOBONamespace>GAZ</oboInOwl:hasOBONamespace>
        <oboInOwl:id>GAZ:00251816</oboInOwl:id>
        <rdfs:label>Ainmiq Swamp</rdfs:label>
    </owl:NamedIndividual>
    


    <!-- http://purl.obolibrary.org/obo/GAZ_00251903 -->

    <owl:NamedIndividual rdf:about="http://purl.obolibrary.org/obo/GAZ_00251903">
        <obo:IAO_0000115>A widening of the Shire River?</obo:IAO_0000115>
        <oboInOwl:hasOBONamespace>GAZ</oboInOwl:hasOBONamespace>
        <oboInOwl:id>GAZ:00251903</oboInOwl:id>
        <rdfs:label>Bangula Lagoon</rdfs:label>
    </owl:NamedIndividual>
    


    <!-- http://purl.obolibrary.org/obo/GAZ_00251905 -->

    <owl:NamedIndividual rdf:about="http://purl.obolibrary.org/obo/GAZ_00251905">
        <obo:RO_0001025 rdf:resource="http://purl.obolibrary.org/obo/GAZ_00041528"/>
        <obo:IAO_0000115>An island.</obo:IAO_0000115>
        <oboInOwl:hasOBONamespace>GAZ</oboInOwl:hasOBONamespace>
        <oboInOwl:id>GAZ:00251905</oboInOwl:id>
        <rdfs:label>Nchisi Island</rdfs:label>
    </owl:NamedIndividual>
    


    <!-- http://purl.obolibrary.org/obo/GAZ_00255602 -->

    <owl:NamedIndividual rdf:about="http://purl.obolibrary.org/obo/GAZ_00255602">
        <obo:IAO_0000115>A river that carries the overspill from Lake Muhazi.</obo:IAO_0000115>
        <oboInOwl:hasOBONamespace>GAZ</oboInOwl:hasOBONamespace>
        <oboInOwl:id>GAZ:00255602</oboInOwl:id>
        <rdfs:label>Nyabugogo River</rdfs:label>
    </owl:NamedIndividual>
    


    <!-- http://purl.obolibrary.org/obo/GAZ_00255604 -->

    <owl:NamedIndividual rdf:about="http://purl.obolibrary.org/obo/GAZ_00255604">
        <obo:RO_0001025 rdf:resource="http://purl.obolibrary.org/obo/GAZ_00053534"/>
        <obo:IAO_0000115>A crater lake.</obo:IAO_0000115>
        <oboInOwl:hasOBONamespace>GAZ</oboInOwl:hasOBONamespace>
        <oboInOwl:id>GAZ:00255604</oboInOwl:id>
        <rdfs:label>Mount Bisoke Lake</rdfs:label>
    </owl:NamedIndividual>
    


    <!-- http://purl.obolibrary.org/obo/GAZ_00255605 -->

    <owl:NamedIndividual rdf:about="http://purl.obolibrary.org/obo/GAZ_00255605">
        <obo:RO_0001025 rdf:resource="http://purl.obolibrary.org/obo/GAZ_00053526"/>
        <obo:IAO_0000115>A crater lake.</obo:IAO_0000115>
        <oboInOwl:hasOBONamespace>GAZ</oboInOwl:hasOBONamespace>
        <oboInOwl:id>GAZ:00255605</oboInOwl:id>
        <rdfs:label>Mount Muhabura Lake</rdfs:label>
    </owl:NamedIndividual>
    


    <!-- http://purl.obolibrary.org/obo/GAZ_00256741 -->

    <owl:NamedIndividual rdf:about="http://purl.obolibrary.org/obo/GAZ_00256741">
        <obo:IAO_0000115>A river.</obo:IAO_0000115>
        <oboInOwl:hasOBONamespace>GAZ</oboInOwl:hasOBONamespace>
        <oboInOwl:id>GAZ:00256741</oboInOwl:id>
        <rdfs:label>Ziuwe River</rdfs:label>
    </owl:NamedIndividual>
    


    <!-- http://purl.obolibrary.org/obo/GAZ_00256743 -->

    <owl:NamedIndividual rdf:about="http://purl.obolibrary.org/obo/GAZ_00256743">
        <obo:RO_0001025 rdf:resource="http://purl.obolibrary.org/obo/GAZ_00256741"/>
        <obo:IAO_0000115>A lake.</obo:IAO_0000115>
        <oboInOwl:hasOBONamespace>GAZ</oboInOwl:hasOBONamespace>
        <oboInOwl:id>GAZ:00256743</oboInOwl:id>
        <rdfs:label>Lake Sagara</rdfs:label>
    </owl:NamedIndividual>
    


    <!-- http://purl.obolibrary.org/obo/GAZ_00260236 -->

    <owl:NamedIndividual rdf:about="http://purl.obolibrary.org/obo/GAZ_00260236">
        <obo:RO_0001025 rdf:resource="http://purl.obolibrary.org/obo/GAZ_00015452"/>
        <obo:IAO_0000115>An island. S of Vumba Island.</obo:IAO_0000115>
        <oboInOwl:hasOBONamespace>GAZ</oboInOwl:hasOBONamespace>
        <oboInOwl:id>GAZ:00260236</oboInOwl:id>
        <rdfs:label>Sagitu Island</rdfs:label>
    </owl:NamedIndividual>
    


    <!-- http://purl.obolibrary.org/obo/GAZ_00260237 -->

    <owl:NamedIndividual rdf:about="http://purl.obolibrary.org/obo/GAZ_00260237">
        <obo:RO_0001025 rdf:resource="http://purl.obolibrary.org/obo/GAZ_00015345"/>
        <obo:RO_0001025 rdf:resource="http://purl.obolibrary.org/obo/GAZ_00015452"/>
        <obo:IAO_0000115>A bay.</obo:IAO_0000115>
        <oboInOwl:hasOBONamespace>GAZ</oboInOwl:hasOBONamespace>
        <oboInOwl:id>GAZ:00260237</oboInOwl:id>
        <rdfs:label>Sango Bay</rdfs:label>
    </owl:NamedIndividual>
    


    <!-- http://purl.obolibrary.org/obo/GAZ_00260238 -->

    <owl:NamedIndividual rdf:about="http://purl.obolibrary.org/obo/GAZ_00260238">
        <obo:RO_0001025 rdf:resource="http://purl.obolibrary.org/obo/GAZ_00005378"/>
        <obo:RO_0001025 rdf:resource="http://purl.obolibrary.org/obo/GAZ_00015452"/>
        <obo:IAO_0000115>A channel N of Bugala Island.</obo:IAO_0000115>
        <oboInOwl:hasOBONamespace>GAZ</oboInOwl:hasOBONamespace>
        <oboInOwl:id>GAZ:00260238</oboInOwl:id>
        <rdfs:label>Salisbury Channel</rdfs:label>
    </owl:NamedIndividual>
    


    <!-- http://purl.obolibrary.org/obo/GAZ_00260252 -->

    <owl:NamedIndividual rdf:about="http://purl.obolibrary.org/obo/GAZ_00260252">
        <obo:RO_0001025 rdf:resource="http://purl.obolibrary.org/obo/GAZ_00015345"/>
        <obo:IAO_0000115>A wetland. A complex of lakes and swamps. Located 33 km ESE of Mbara.</obo:IAO_0000115>
        <oboInOwl:hasOBONamespace>GAZ</oboInOwl:hasOBONamespace>
        <oboInOwl:id>GAZ:00260252</oboInOwl:id>
        <rdfs:label>Kijanebalola Lake/Swamp Complex</rdfs:label>
    </owl:NamedIndividual>
    


    <!-- http://purl.obolibrary.org/obo/GAZ_00260255 -->

    <owl:NamedIndividual rdf:about="http://purl.obolibrary.org/obo/GAZ_00260255">
        <obo:RO_0001025 rdf:resource="http://purl.obolibrary.org/obo/GAZ_00260252"/>
        <obo:IAO_0000115>A freshwater lake.</obo:IAO_0000115>
        <oboInOwl:hasOBONamespace>GAZ</oboInOwl:hasOBONamespace>
        <oboInOwl:id>GAZ:00260255</oboInOwl:id>
        <rdfs:label>Lake Nakivali</rdfs:label>
    </owl:NamedIndividual>
    


    <!-- http://purl.obolibrary.org/obo/GAZ_00260256 -->

    <owl:NamedIndividual rdf:about="http://purl.obolibrary.org/obo/GAZ_00260256">
        <obo:RO_0001025 rdf:resource="http://purl.obolibrary.org/obo/GAZ_00260252"/>
        <obo:IAO_0000115>A freshwater lake.</obo:IAO_0000115>
        <oboInOwl:hasOBONamespace>GAZ</oboInOwl:hasOBONamespace>
        <oboInOwl:id>GAZ:00260256</oboInOwl:id>
        <rdfs:label>Lake Mburo</rdfs:label>
    </owl:NamedIndividual>
    


    <!-- http://purl.obolibrary.org/obo/GAZ_00260257 -->

    <owl:NamedIndividual rdf:about="http://purl.obolibrary.org/obo/GAZ_00260257">
        <obo:RO_0001025 rdf:resource="http://purl.obolibrary.org/obo/GAZ_00260252"/>
        <obo:IAO_0000115>A freshwater lake.</obo:IAO_0000115>
        <oboInOwl:hasOBONamespace>GAZ</oboInOwl:hasOBONamespace>
        <oboInOwl:id>GAZ:00260257</oboInOwl:id>
        <rdfs:label>Lake Kachira</rdfs:label>
    </owl:NamedIndividual>
    


    <!-- http://purl.obolibrary.org/obo/GAZ_00260258 -->

    <owl:NamedIndividual rdf:about="http://purl.obolibrary.org/obo/GAZ_00260258">
        <obo:RO_0001025 rdf:resource="http://purl.obolibrary.org/obo/GAZ_00260252"/>
        <obo:IAO_0000115>A freshwater lake.</obo:IAO_0000115>
        <oboInOwl:hasOBONamespace>GAZ</oboInOwl:hasOBONamespace>
        <oboInOwl:id>GAZ:00260258</oboInOwl:id>
        <rdfs:label>Lake Kijanebalola</rdfs:label>
    </owl:NamedIndividual>
    


    <!-- http://purl.obolibrary.org/obo/GAZ_00260259 -->

    <owl:NamedIndividual rdf:about="http://purl.obolibrary.org/obo/GAZ_00260259">
        <obo:RO_0001025 rdf:resource="http://purl.obolibrary.org/obo/GAZ_00260252"/>
        <obo:IAO_0000115>A freshwater lake.</obo:IAO_0000115>
        <oboInOwl:hasOBONamespace>GAZ</oboInOwl:hasOBONamespace>
        <oboInOwl:id>GAZ:00260259</oboInOwl:id>
        <rdfs:label>Lake Kiretwa</rdfs:label>
    </owl:NamedIndividual>
    


    <!-- http://purl.obolibrary.org/obo/GAZ_00260260 -->

    <owl:NamedIndividual rdf:about="http://purl.obolibrary.org/obo/GAZ_00260260">
        <obo:RO_0001025 rdf:resource="http://purl.obolibrary.org/obo/GAZ_00260252"/>
        <obo:IAO_0000115>A freshwater lake.</obo:IAO_0000115>
        <oboInOwl:hasOBONamespace>GAZ</oboInOwl:hasOBONamespace>
        <oboInOwl:id>GAZ:00260260</oboInOwl:id>
        <rdfs:label>Lake Kasasa</rdfs:label>
    </owl:NamedIndividual>
    


    <!-- http://purl.obolibrary.org/obo/GAZ_00260261 -->

    <owl:NamedIndividual rdf:about="http://purl.obolibrary.org/obo/GAZ_00260261">
        <obo:RO_0001025 rdf:resource="http://purl.obolibrary.org/obo/GAZ_00260252"/>
        <obo:IAO_0000115>A freshwater lake.</obo:IAO_0000115>
        <oboInOwl:hasOBONamespace>GAZ</oboInOwl:hasOBONamespace>
        <oboInOwl:id>GAZ:00260261</oboInOwl:id>
        <rdfs:label>Lake Mutukura</rdfs:label>
    </owl:NamedIndividual>
    


    <!-- http://purl.obolibrary.org/obo/GAZ_00260262 -->

    <owl:NamedIndividual rdf:about="http://purl.obolibrary.org/obo/GAZ_00260262">
        <obo:RO_0001025 rdf:resource="http://purl.obolibrary.org/obo/GAZ_00260252"/>
        <obo:IAO_0000115>A freshwater lake.</obo:IAO_0000115>
        <oboInOwl:hasOBONamespace>GAZ</oboInOwl:hasOBONamespace>
        <oboInOwl:id>GAZ:00260262</oboInOwl:id>
        <rdfs:label>Lake Kazuma</rdfs:label>
    </owl:NamedIndividual>
    


    <!-- http://purl.obolibrary.org/obo/GAZ_00260263 -->

    <owl:NamedIndividual rdf:about="http://purl.obolibrary.org/obo/GAZ_00260263">
        <obo:RO_0001025 rdf:resource="http://purl.obolibrary.org/obo/GAZ_00260252"/>
        <obo:IAO_0000115>A freshwater lake.</obo:IAO_0000115>
        <oboInOwl:hasOBONamespace>GAZ</oboInOwl:hasOBONamespace>
        <oboInOwl:id>GAZ:00260263</oboInOwl:id>
        <rdfs:label>Lake Mishera</rdfs:label>
    </owl:NamedIndividual>
    


    <!-- http://purl.obolibrary.org/obo/GAZ_00260264 -->

    <owl:NamedIndividual rdf:about="http://purl.obolibrary.org/obo/GAZ_00260264">
        <obo:RO_0001025 rdf:resource="http://purl.obolibrary.org/obo/GAZ_00260252"/>
        <obo:IAO_0000115>A freshwater lake.</obo:IAO_0000115>
        <oboInOwl:hasOBONamespace>GAZ</oboInOwl:hasOBONamespace>
        <oboInOwl:id>GAZ:00260264</oboInOwl:id>
        <rdfs:label>Lake Ruma</rdfs:label>
    </owl:NamedIndividual>
    


    <!-- http://purl.obolibrary.org/obo/GAZ_00260265 -->

    <owl:NamedIndividual rdf:about="http://purl.obolibrary.org/obo/GAZ_00260265">
        <obo:RO_0001025 rdf:resource="http://purl.obolibrary.org/obo/GAZ_00260252"/>
        <obo:IAO_0000115>A freshwater lake.</obo:IAO_0000115>
        <oboInOwl:hasOBONamespace>GAZ</oboInOwl:hasOBONamespace>
        <oboInOwl:id>GAZ:00260265</oboInOwl:id>
        <rdfs:label>Lake Karitima</rdfs:label>
    </owl:NamedIndividual>
    


    <!-- http://purl.obolibrary.org/obo/GAZ_00260266 -->

    <owl:NamedIndividual rdf:about="http://purl.obolibrary.org/obo/GAZ_00260266">
        <obo:RO_0001025 rdf:resource="http://purl.obolibrary.org/obo/GAZ_00260252"/>
        <obo:IAO_0000115>A freshwater lake.</obo:IAO_0000115>
        <oboInOwl:hasOBONamespace>GAZ</oboInOwl:hasOBONamespace>
        <oboInOwl:id>GAZ:00260266</oboInOwl:id>
        <rdfs:label>Lake Bwara</rdfs:label>
    </owl:NamedIndividual>
    


    <!-- http://purl.obolibrary.org/obo/GAZ_00260267 -->

    <owl:NamedIndividual rdf:about="http://purl.obolibrary.org/obo/GAZ_00260267">
        <obo:RO_0001025 rdf:resource="http://purl.obolibrary.org/obo/GAZ_00260252"/>
        <obo:IAO_0000115>A freshwater lake.</obo:IAO_0000115>
        <oboInOwl:hasOBONamespace>GAZ</oboInOwl:hasOBONamespace>
        <oboInOwl:id>GAZ:00260267</oboInOwl:id>
        <rdfs:label>Lake Karunga</rdfs:label>
    </owl:NamedIndividual>
    


    <!-- http://purl.obolibrary.org/obo/GAZ_00260277 -->

    <owl:NamedIndividual rdf:about="http://purl.obolibrary.org/obo/GAZ_00260277">
        <obo:RO_0001025 rdf:resource="http://purl.obolibrary.org/obo/GAZ_00015405"/>
        <obo:RO_0001025 rdf:resource="http://purl.obolibrary.org/obo/GAZ_00076731"/>
        <obo:IAO_0000115>A crater lake.</obo:IAO_0000115>
        <oboInOwl:hasOBONamespace>GAZ</oboInOwl:hasOBONamespace>
        <oboInOwl:id>GAZ:00260277</oboInOwl:id>
        <rdfs:label>Lake Bagusa</rdfs:label>
    </owl:NamedIndividual>
    


    <!-- http://purl.obolibrary.org/obo/GAZ_00260278 -->

    <owl:NamedIndividual rdf:about="http://purl.obolibrary.org/obo/GAZ_00260278">
        <obo:RO_0001025 rdf:resource="http://purl.obolibrary.org/obo/GAZ_00015405"/>
        <obo:IAO_0000115>A crater lake.</obo:IAO_0000115>
        <oboInOwl:hasOBONamespace>GAZ</oboInOwl:hasOBONamespace>
        <oboInOwl:id>GAZ:00260278</oboInOwl:id>
        <rdfs:label>Lake Kyamwiga</rdfs:label>
    </owl:NamedIndividual>
    


    <!-- http://purl.obolibrary.org/obo/GAZ_00260279 -->

    <owl:NamedIndividual rdf:about="http://purl.obolibrary.org/obo/GAZ_00260279">
        <obo:RO_0001025 rdf:resource="http://purl.obolibrary.org/obo/GAZ_00015405"/>
        <obo:IAO_0000115>A crater lake.</obo:IAO_0000115>
        <oboInOwl:hasOBONamespace>GAZ</oboInOwl:hasOBONamespace>
        <oboInOwl:id>GAZ:00260279</oboInOwl:id>
        <rdfs:label>Lake Bugwagi</rdfs:label>
    </owl:NamedIndividual>
    


    <!-- http://purl.obolibrary.org/obo/GAZ_00260280 -->

    <owl:NamedIndividual rdf:about="http://purl.obolibrary.org/obo/GAZ_00260280">
        <obo:RO_0001025 rdf:resource="http://purl.obolibrary.org/obo/GAZ_00015405"/>
        <obo:IAO_0000115>A crater lake.</obo:IAO_0000115>
        <oboInOwl:hasOBONamespace>GAZ</oboInOwl:hasOBONamespace>
        <oboInOwl:id>GAZ:00260280</oboInOwl:id>
        <rdfs:label>Lake Katinda</rdfs:label>
    </owl:NamedIndividual>
    


    <!-- http://purl.obolibrary.org/obo/GAZ_00260281 -->

    <owl:NamedIndividual rdf:about="http://purl.obolibrary.org/obo/GAZ_00260281">
        <obo:RO_0001025 rdf:resource="http://purl.obolibrary.org/obo/GAZ_00015405"/>
        <obo:IAO_0000115>A crater lake.</obo:IAO_0000115>
        <oboInOwl:hasOBONamespace>GAZ</oboInOwl:hasOBONamespace>
        <oboInOwl:id>GAZ:00260281</oboInOwl:id>
        <rdfs:label>Lake Mirambi</rdfs:label>
    </owl:NamedIndividual>
    


    <!-- http://purl.obolibrary.org/obo/GAZ_00260282 -->

    <owl:NamedIndividual rdf:about="http://purl.obolibrary.org/obo/GAZ_00260282">
        <obo:RO_0001025 rdf:resource="http://purl.obolibrary.org/obo/GAZ_00015405"/>
        <obo:IAO_0000115>A crater lake.</obo:IAO_0000115>
        <oboInOwl:hasOBONamespace>GAZ</oboInOwl:hasOBONamespace>
        <oboInOwl:id>GAZ:00260282</oboInOwl:id>
        <rdfs:label>Lake Moseche</rdfs:label>
    </owl:NamedIndividual>
    


    <!-- http://purl.obolibrary.org/obo/GAZ_00260283 -->

    <owl:NamedIndividual rdf:about="http://purl.obolibrary.org/obo/GAZ_00260283">
        <obo:RO_0001025 rdf:resource="http://purl.obolibrary.org/obo/GAZ_00015405"/>
        <obo:IAO_0000115>A crater lake.</obo:IAO_0000115>
        <oboInOwl:hasOBONamespace>GAZ</oboInOwl:hasOBONamespace>
        <oboInOwl:id>GAZ:00260283</oboInOwl:id>
        <rdfs:label>Lake Mshenyi</rdfs:label>
    </owl:NamedIndividual>
    


    <!-- http://purl.obolibrary.org/obo/GAZ_00260284 -->

    <owl:NamedIndividual rdf:about="http://purl.obolibrary.org/obo/GAZ_00260284">
        <obo:RO_0001025 rdf:resource="http://purl.obolibrary.org/obo/GAZ_00015405"/>
        <obo:IAO_0000115>A crater lake.</obo:IAO_0000115>
        <oboInOwl:hasOBONamespace>GAZ</oboInOwl:hasOBONamespace>
        <oboInOwl:id>GAZ:00260284</oboInOwl:id>
        <rdfs:label>Lake Chibera</rdfs:label>
    </owl:NamedIndividual>
    


    <!-- http://purl.obolibrary.org/obo/GAZ_00260285 -->

    <owl:NamedIndividual rdf:about="http://purl.obolibrary.org/obo/GAZ_00260285">
        <obo:RO_0001025 rdf:resource="http://purl.obolibrary.org/obo/GAZ_00015405"/>
        <obo:IAO_0000115>A crater lake.</obo:IAO_0000115>
        <oboInOwl:hasOBONamespace>GAZ</oboInOwl:hasOBONamespace>
        <oboInOwl:id>GAZ:00260285</oboInOwl:id>
        <rdfs:label>Lake Mugogo</rdfs:label>
    </owl:NamedIndividual>
    


    <!-- http://purl.obolibrary.org/obo/GAZ_00260286 -->

    <owl:NamedIndividual rdf:about="http://purl.obolibrary.org/obo/GAZ_00260286">
        <obo:RO_0001025 rdf:resource="http://purl.obolibrary.org/obo/GAZ_00015405"/>
        <obo:IAO_0000115>A crater lake.</obo:IAO_0000115>
        <oboInOwl:hasOBONamespace>GAZ</oboInOwl:hasOBONamespace>
        <oboInOwl:id>GAZ:00260286</oboInOwl:id>
        <rdfs:label>Lake Kyasanduka</rdfs:label>
    </owl:NamedIndividual>
    


    <!-- http://purl.obolibrary.org/obo/GAZ_00260287 -->

    <owl:NamedIndividual rdf:about="http://purl.obolibrary.org/obo/GAZ_00260287">
        <obo:RO_0001025 rdf:resource="http://purl.obolibrary.org/obo/GAZ_00015405"/>
        <obo:IAO_0000115>A crater lake.</obo:IAO_0000115>
        <oboInOwl:hasOBONamespace>GAZ</oboInOwl:hasOBONamespace>
        <oboInOwl:id>GAZ:00260287</oboInOwl:id>
        <rdfs:label>Lake Murunuli</rdfs:label>
    </owl:NamedIndividual>
    


    <!-- http://purl.obolibrary.org/obo/GAZ_00260288 -->

    <owl:NamedIndividual rdf:about="http://purl.obolibrary.org/obo/GAZ_00260288">
        <obo:RO_0001025 rdf:resource="http://purl.obolibrary.org/obo/GAZ_00015405"/>
        <obo:RO_0001025 rdf:resource="http://purl.obolibrary.org/obo/GAZ_00076731"/>
        <obo:IAO_0000115>A crater lake.</obo:IAO_0000115>
        <oboInOwl:hasOBONamespace>GAZ</oboInOwl:hasOBONamespace>
        <oboInOwl:id>GAZ:00260288</oboInOwl:id>
        <rdfs:label>Lake Nyamusingire</rdfs:label>
    </owl:NamedIndividual>
    


    <!-- http://purl.obolibrary.org/obo/GAZ_00260289 -->

    <owl:NamedIndividual rdf:about="http://purl.obolibrary.org/obo/GAZ_00260289">
        <obo:RO_0001025 rdf:resource="http://purl.obolibrary.org/obo/GAZ_00015394"/>
        <obo:RO_0001025 rdf:resource="http://purl.obolibrary.org/obo/GAZ_00076731"/>
        <obo:IAO_0000115>A crater lake situated west of Lake George, just north of the Kazinga Channel and between Lakes George and Edward.</obo:IAO_0000115>
        <oboInOwl:hasOBONamespace>GAZ</oboInOwl:hasOBONamespace>
        <oboInOwl:id>GAZ:00260289</oboInOwl:id>
        <rdfs:label>Lake Kitagata</rdfs:label>
    </owl:NamedIndividual>
    


    <!-- http://purl.obolibrary.org/obo/GAZ_00260290 -->

    <owl:NamedIndividual rdf:about="http://purl.obolibrary.org/obo/GAZ_00260290">
        <obo:RO_0001025 rdf:resource="http://purl.obolibrary.org/obo/GAZ_00015394"/>
        <obo:RO_0001025 rdf:resource="http://purl.obolibrary.org/obo/GAZ_00076731"/>
        <obo:IAO_0000115>A crater lake situated west of Lake George, just north of the Kazinga Channel and between Lakes George and Edward.</obo:IAO_0000115>
        <oboInOwl:hasOBONamespace>GAZ</oboInOwl:hasOBONamespace>
        <oboInOwl:id>GAZ:00260290</oboInOwl:id>
        <rdfs:label>Lake Murunuli</rdfs:label>
    </owl:NamedIndividual>
    


    <!-- http://purl.obolibrary.org/obo/GAZ_00260291 -->

    <owl:NamedIndividual rdf:about="http://purl.obolibrary.org/obo/GAZ_00260291">
        <obo:RO_0001025 rdf:resource="http://purl.obolibrary.org/obo/GAZ_00015394"/>
        <obo:RO_0001025 rdf:resource="http://purl.obolibrary.org/obo/GAZ_00076731"/>
        <obo:IAO_0000115>A crater lake situated west of Lake George, just north of the Kazinga Channel and between Lakes George and Edward.</obo:IAO_0000115>
        <oboInOwl:hasOBONamespace>GAZ</oboInOwl:hasOBONamespace>
        <oboInOwl:id>GAZ:00260291</oboInOwl:id>
        <rdfs:label>Lake Nyamunuka</rdfs:label>
    </owl:NamedIndividual>
    


    <!-- http://purl.obolibrary.org/obo/GAZ_00260292 -->

    <owl:NamedIndividual rdf:about="http://purl.obolibrary.org/obo/GAZ_00260292">
        <rdf:type rdf:resource="http://purl.obolibrary.org/obo/ENVO_00000475"/>
        <obo:RO_0001025 rdf:resource="http://purl.obolibrary.org/obo/GAZ_00058791"/>
        <obo:IAO_0000115>An arm of Lake Kyoga.</obo:IAO_0000115>
        <oboInOwl:hasOBONamespace>GAZ</oboInOwl:hasOBONamespace>
        <oboInOwl:id>GAZ:00260292</oboInOwl:id>
        <rdfs:label>Mpologoma Arm</rdfs:label>
    </owl:NamedIndividual>
    


    <!-- http://purl.obolibrary.org/obo/GAZ_00260963 -->

    <owl:NamedIndividual rdf:about="http://purl.obolibrary.org/obo/GAZ_00260963">
        <obo:RO_0001025 rdf:resource="http://purl.obolibrary.org/obo/GAZ_00041530"/>
        <obo:IAO_0000115>An island.</obo:IAO_0000115>
        <oboInOwl:hasOBONamespace>GAZ</oboInOwl:hasOBONamespace>
        <oboInOwl:id>GAZ:00260963</oboInOwl:id>
        <rdfs:label>N&apos;Kole Island</rdfs:label>
    </owl:NamedIndividual>
    


    <!-- http://purl.obolibrary.org/obo/GAZ_00260964 -->

    <owl:NamedIndividual rdf:about="http://purl.obolibrary.org/obo/GAZ_00260964">
        <obo:RO_0001025 rdf:resource="http://purl.obolibrary.org/obo/GAZ_00058782"/>
        <obo:IAO_0000115>A lake lagoon in Zambia. It is in the Luapula River swamps south of Lake Mweru, in the Luapula Province of Zambia.</obo:IAO_0000115>
        <oboInOwl:hasOBONamespace>GAZ</oboInOwl:hasOBONamespace>
        <oboInOwl:id>GAZ:00260964</oboInOwl:id>
        <rdfs:label>Pembe Lagoon</rdfs:label>
    </owl:NamedIndividual>
    


    <!-- http://purl.obolibrary.org/obo/GAZ_00260965 -->

    <owl:NamedIndividual rdf:about="http://purl.obolibrary.org/obo/GAZ_00260965">
        <obo:RO_0001025 rdf:resource="http://purl.obolibrary.org/obo/GAZ_00058782"/>
        <obo:IAO_0000115>A lake on the Luapula Floodplain.</obo:IAO_0000115>
        <oboInOwl:hasOBONamespace>GAZ</oboInOwl:hasOBONamespace>
        <oboInOwl:id>GAZ:00260965</oboInOwl:id>
        <rdfs:label>Lake Kuswa</rdfs:label>
    </owl:NamedIndividual>
    


    <!-- http://purl.obolibrary.org/obo/GAZ_00260966 -->

    <owl:NamedIndividual rdf:about="http://purl.obolibrary.org/obo/GAZ_00260966">
        <obo:RO_0001025 rdf:resource="http://purl.obolibrary.org/obo/GAZ_00058782"/>
        <obo:IAO_0000115>A lake on the Luapula Floodplain.</obo:IAO_0000115>
        <oboInOwl:hasOBONamespace>GAZ</oboInOwl:hasOBONamespace>
        <oboInOwl:id>GAZ:00260966</oboInOwl:id>
        <rdfs:label>Lake Kitshomponshi</rdfs:label>
    </owl:NamedIndividual>
    


    <!-- http://purl.obolibrary.org/obo/GAZ_00260967 -->

    <owl:NamedIndividual rdf:about="http://purl.obolibrary.org/obo/GAZ_00260967">
        <obo:RO_0001025 rdf:resource="http://purl.obolibrary.org/obo/GAZ_00058782"/>
        <obo:IAO_0000115>A lake on the Luapula Floodplain.</obo:IAO_0000115>
        <oboInOwl:hasOBONamespace>GAZ</oboInOwl:hasOBONamespace>
        <oboInOwl:id>GAZ:00260967</oboInOwl:id>
        <rdfs:label>Lake Kifukula</rdfs:label>
    </owl:NamedIndividual>
    


    <!-- http://purl.obolibrary.org/obo/GAZ_00260968 -->

    <owl:NamedIndividual rdf:about="http://purl.obolibrary.org/obo/GAZ_00260968">
        <obo:RO_0001025 rdf:resource="http://purl.obolibrary.org/obo/GAZ_00058782"/>
        <obo:IAO_0000115>A lake on the Luapula Floodplain.</obo:IAO_0000115>
        <oboInOwl:hasOBONamespace>GAZ</oboInOwl:hasOBONamespace>
        <oboInOwl:id>GAZ:00260968</oboInOwl:id>
        <rdfs:label>Lake Kainsa</rdfs:label>
    </owl:NamedIndividual>
    


    <!-- http://purl.obolibrary.org/obo/GAZ_00260969 -->

    <owl:NamedIndividual rdf:about="http://purl.obolibrary.org/obo/GAZ_00260969">
        <obo:RO_0001025 rdf:resource="http://purl.obolibrary.org/obo/GAZ_00058782"/>
        <obo:IAO_0000115>A lake on the Luapula Floodplain.</obo:IAO_0000115>
        <oboInOwl:hasOBONamespace>GAZ</oboInOwl:hasOBONamespace>
        <oboInOwl:id>GAZ:00260969</oboInOwl:id>
        <rdfs:label>Lake Kinseneka</rdfs:label>
    </owl:NamedIndividual>
    


    <!-- http://purl.obolibrary.org/obo/GAZ_00260970 -->

    <owl:NamedIndividual rdf:about="http://purl.obolibrary.org/obo/GAZ_00260970">
        <obo:RO_0001025 rdf:resource="http://purl.obolibrary.org/obo/GAZ_00041532"/>
        <obo:IAO_0000115>An island.</obo:IAO_0000115>
        <oboInOwl:hasOBONamespace>GAZ</oboInOwl:hasOBONamespace>
        <oboInOwl:id>GAZ:00260970</oboInOwl:id>
        <rdfs:label>Katima Island</rdfs:label>
    </owl:NamedIndividual>
    


    <!-- http://purl.obolibrary.org/obo/GAZ_00281432 -->

    <owl:NamedIndividual rdf:about="http://purl.obolibrary.org/obo/GAZ_00281432">
        <obo:RO_0001025 rdf:resource="http://purl.obolibrary.org/obo/GAZ_00124306"/>
        <obo:IAO_0000115>An archeological site. A Late Stone Age site in Mau Escarpment of Kenya.</obo:IAO_0000115>
        <oboInOwl:hasOBONamespace>GAZ</oboInOwl:hasOBONamespace>
        <oboInOwl:id>GAZ:00281432</oboInOwl:id>
        <rdfs:label>Enkapune Ya Muto</rdfs:label>
    </owl:NamedIndividual>
    


    <!-- http://purl.obolibrary.org/obo/GAZ_00281451 -->

    <owl:NamedIndividual rdf:about="http://purl.obolibrary.org/obo/GAZ_00281451">
        <obo:IAO_0000115>A single drop waterfall on the border of Zambia and Tanzania at the southeast end of Lake Tanganyika.</obo:IAO_0000115>
        <oboInOwl:hasOBONamespace>GAZ</oboInOwl:hasOBONamespace>
        <oboInOwl:id>GAZ:00281451</oboInOwl:id>
        <rdfs:label>Kalambo Falls</rdfs:label>
    </owl:NamedIndividual>
    


    <!-- http://purl.obolibrary.org/obo/GAZ_00604691 -->

    <owl:NamedIndividual rdf:about="http://purl.obolibrary.org/obo/GAZ_00604691">
        <obo:RO_0001025 rdf:resource="http://purl.obolibrary.org/obo/GAZ_00236543"/>
        <obo:IAO_0000115>A miitary airport.</obo:IAO_0000115>
        <oboInOwl:hasOBONamespace>GAZ</oboInOwl:hasOBONamespace>
        <oboInOwl:id>GAZ:00604691</oboInOwl:id>
        <rdfs:label>Nakasongola Airport</rdfs:label>
    </owl:NamedIndividual>
    


    <!-- 
    ///////////////////////////////////////////////////////////////////////////////////////
    //
    // Annotations
    //
    ///////////////////////////////////////////////////////////////////////////////////////
     -->

    <rdf:Description rdf:about="http://purl.obolibrary.org/obo/GAZ_00005373">
        <oboInOwl:hasOBONamespace>GAZ</oboInOwl:hasOBONamespace>
        <oboInOwl:id>GAZ:00005373</oboInOwl:id>
        <rdfs:label>Region (Uganda)</rdfs:label>
    </rdf:Description>
    <rdf:Description rdf:about="http://purl.obolibrary.org/obo/GAZ_00005374">
        <rdfs:label>Western Region</rdfs:label>
        <oboInOwl:hasOBONamespace>GAZ</oboInOwl:hasOBONamespace>
        <oboInOwl:id>GAZ:00005374</oboInOwl:id>
        <obo:IAO_0000115>An administrative Region of Uganda.</obo:IAO_0000115>
    </rdf:Description>
    <rdf:Description rdf:about="http://purl.obolibrary.org/obo/GAZ_00005375">
        <obo:IAO_0000115>An administrative Region of Uganda.</obo:IAO_0000115>
        <oboInOwl:hasOBONamespace>GAZ</oboInOwl:hasOBONamespace>
        <oboInOwl:id>GAZ:00005375</oboInOwl:id>
        <rdfs:label>Northern Region</rdfs:label>
    </rdf:Description>
    <rdf:Description rdf:about="http://purl.obolibrary.org/obo/GAZ_00005376">
        <rdfs:label>Eastern Region</rdfs:label>
        <obo:IAO_0000115>An administrative Region of Uganda.</obo:IAO_0000115>
        <oboInOwl:hasOBONamespace>GAZ</oboInOwl:hasOBONamespace>
        <oboInOwl:id>GAZ:00005376</oboInOwl:id>
    </rdf:Description>
    <rdf:Description rdf:about="http://purl.obolibrary.org/obo/GAZ_00005377">
        <obo:IAO_0000115>An administrative Region of Uganda.</obo:IAO_0000115>
        <rdfs:label>Central Region</rdfs:label>
        <oboInOwl:hasOBONamespace>GAZ</oboInOwl:hasOBONamespace>
        <oboInOwl:id>GAZ:00005377</oboInOwl:id>
    </rdf:Description>
    <rdf:Description rdf:about="http://purl.obolibrary.org/obo/GAZ_00005381">
        <rdfs:label>Masaka</rdfs:label>
        <obo:IAO_0000115>A populated place.</obo:IAO_0000115>
        <oboInOwl:hasOBONamespace>GAZ</oboInOwl:hasOBONamespace>
        <oboInOwl:id>GAZ:00005381</oboInOwl:id>
    </rdf:Description>
    <rdf:Description rdf:about="http://purl.obolibrary.org/obo/GAZ_00005382">
        <oboInOwl:id>GAZ:00005382</oboInOwl:id>
        <oboInOwl:hasOBONamespace>GAZ</oboInOwl:hasOBONamespace>
        <rdfs:label>populated place, Uganda</rdfs:label>
    </rdf:Description>
    <rdf:Description rdf:about="http://purl.obolibrary.org/obo/GAZ_00009914">
        <rdfs:label>Gulu</rdfs:label>
        <obo:IAO_0000115>A populated place. A city in northern Uganda. It is the commercial and administrative centre of Gulu District.</obo:IAO_0000115>
        <oboInOwl:id>GAZ:00009914</oboInOwl:id>
        <oboInOwl:hasOBONamespace>GAZ</oboInOwl:hasOBONamespace>
    </rdf:Description>
    <rdf:Description rdf:about="http://purl.obolibrary.org/obo/GAZ_00009916">
        <rdfs:label>Masindi</rdfs:label>
        <oboInOwl:id>GAZ:00009916</oboInOwl:id>
        <obo:IAO_0000115>A populated place.</obo:IAO_0000115>
        <oboInOwl:hasOBONamespace>GAZ</oboInOwl:hasOBONamespace>
    </rdf:Description>
    <rdf:Description rdf:about="http://purl.obolibrary.org/obo/GAZ_00009918">
        <rdfs:label>Mbarara</rdfs:label>
        <oboInOwl:id>GAZ:00009918</oboInOwl:id>
        <obo:IAO_0000115>A populated place.</obo:IAO_0000115>
        <oboInOwl:hasOBONamespace>GAZ</oboInOwl:hasOBONamespace>
    </rdf:Description>
    <rdf:Description rdf:about="http://purl.obolibrary.org/obo/GAZ_00015413">
        <oboInOwl:id>GAZ:00015413</oboInOwl:id>
        <oboInOwl:hasOBONamespace>GAZ</oboInOwl:hasOBONamespace>
        <obo:IAO_0000115>A county (third-level administrative division) of Uganda.</obo:IAO_0000115>
        <rdfs:label>Municipality of Entebbe</rdfs:label>
    </rdf:Description>
</rdf:RDF>



<!-- Generated by the OWL API (version 4.5.6) https://github.com/owlcs/owlapi -->

