<?xml version="1.0"?>
<rdf:RDF xmlns="http://purl.obolibrary.org/obo/gaz/subsets/countries/United_Arab_Emirates.owl#"
     xml:base="http://purl.obolibrary.org/obo/gaz/subsets/countries/United_Arab_Emirates.owl"
     xmlns:obo="http://purl.obolibrary.org/obo/"
     xmlns:owl="http://www.w3.org/2002/07/owl#"
     xmlns:rdf="http://www.w3.org/1999/02/22-rdf-syntax-ns#"
     xmlns:xml="http://www.w3.org/XML/1998/namespace"
     xmlns:xsd="http://www.w3.org/2001/XMLSchema#"
     xmlns:rdfs="http://www.w3.org/2000/01/rdf-schema#"
     xmlns:oboInOwl="http://www.geneontology.org/formats/oboInOwl#">
    <owl:Ontology rdf:about="http://purl.obolibrary.org/obo/gaz/subsets/countries/United_Arab_Emirates.owl">
        <owl:imports rdf:resource="http://purl.obolibrary.org/obo/gaz/imports/envo_import.owl"/>
        <owl:imports rdf:resource="http://purl.obolibrary.org/obo/gaz/imports/ro_import.owl"/>
    </owl:Ontology>
    


    <!-- 
    ///////////////////////////////////////////////////////////////////////////////////////
    //
    // Annotation properties
    //
    ///////////////////////////////////////////////////////////////////////////////////////
     -->

    


    <!-- http://purl.obolibrary.org/obo/IAO_0000115 -->

    <owl:AnnotationProperty rdf:about="http://purl.obolibrary.org/obo/IAO_0000115"/>
    


    <!-- http://www.geneontology.org/formats/oboInOwl#hasOBONamespace -->

    <owl:AnnotationProperty rdf:about="http://www.geneontology.org/formats/oboInOwl#hasOBONamespace"/>
    


    <!-- http://www.geneontology.org/formats/oboInOwl#id -->

    <owl:AnnotationProperty rdf:about="http://www.geneontology.org/formats/oboInOwl#id"/>
    


    <!-- 
    ///////////////////////////////////////////////////////////////////////////////////////
    //
    // Object Properties
    //
    ///////////////////////////////////////////////////////////////////////////////////////
     -->

    


    <!-- http://purl.obolibrary.org/obo/RO_0001025 -->

    <owl:ObjectProperty rdf:about="http://purl.obolibrary.org/obo/RO_0001025"/>
    


    <!-- 
    ///////////////////////////////////////////////////////////////////////////////////////
    //
    // Classes
    //
    ///////////////////////////////////////////////////////////////////////////////////////
     -->

    


    <!-- http://purl.obolibrary.org/obo/ENVO_00000167 -->

    <owl:Class rdf:about="http://purl.obolibrary.org/obo/ENVO_00000167"/>
    


    <!-- http://purl.obolibrary.org/obo/ENVO_00000475 -->

    <owl:Class rdf:about="http://purl.obolibrary.org/obo/ENVO_00000475"/>
    


    <!-- http://purl.obolibrary.org/obo/ENVO_00000856 -->

    <owl:Class rdf:about="http://purl.obolibrary.org/obo/ENVO_00000856"/>
    


    <!-- http://purl.obolibrary.org/obo/GAZ_00005287 -->

    <owl:Class rdf:about="http://purl.obolibrary.org/obo/GAZ_00005287"/>
    


    <!-- http://purl.obolibrary.org/obo/GAZ_00005288 -->

    <owl:Class rdf:about="http://purl.obolibrary.org/obo/GAZ_00005288">
        <rdfs:subClassOf rdf:resource="http://purl.obolibrary.org/obo/GAZ_00005287"/>
    </owl:Class>
    


    <!-- http://purl.obolibrary.org/obo/GAZ_00005289 -->

    <owl:Class rdf:about="http://purl.obolibrary.org/obo/GAZ_00005289">
        <rdfs:subClassOf rdf:resource="http://purl.obolibrary.org/obo/GAZ_00005287"/>
    </owl:Class>
    


    <!-- http://purl.obolibrary.org/obo/GAZ_00005290 -->

    <owl:Class rdf:about="http://purl.obolibrary.org/obo/GAZ_00005290">
        <rdfs:subClassOf rdf:resource="http://purl.obolibrary.org/obo/GAZ_00005287"/>
    </owl:Class>
    


    <!-- http://purl.obolibrary.org/obo/GAZ_00005291 -->

    <owl:Class rdf:about="http://purl.obolibrary.org/obo/GAZ_00005291">
        <rdfs:subClassOf rdf:resource="http://purl.obolibrary.org/obo/GAZ_00005287"/>
    </owl:Class>
    


    <!-- http://purl.obolibrary.org/obo/GAZ_00005292 -->

    <owl:Class rdf:about="http://purl.obolibrary.org/obo/GAZ_00005292">
        <rdfs:subClassOf rdf:resource="http://purl.obolibrary.org/obo/GAZ_00005287"/>
    </owl:Class>
    


    <!-- http://purl.obolibrary.org/obo/GAZ_00005293 -->

    <owl:Class rdf:about="http://purl.obolibrary.org/obo/GAZ_00005293">
        <rdfs:subClassOf rdf:resource="http://purl.obolibrary.org/obo/GAZ_00005287"/>
    </owl:Class>
    


    <!-- http://purl.obolibrary.org/obo/GAZ_00005294 -->

    <owl:Class rdf:about="http://purl.obolibrary.org/obo/GAZ_00005294">
        <rdfs:subClassOf rdf:resource="http://purl.obolibrary.org/obo/GAZ_00005287"/>
    </owl:Class>
    


    <!-- 
    ///////////////////////////////////////////////////////////////////////////////////////
    //
    // Individuals
    //
    ///////////////////////////////////////////////////////////////////////////////////////
     -->

    


    <!-- http://purl.obolibrary.org/obo/GAZ_00005282 -->

    <owl:NamedIndividual rdf:about="http://purl.obolibrary.org/obo/GAZ_00005282">
        <obo:IAO_0000115>A Middle Eastern federation of seven states situated in the southeast of the Arabian Peninsula in Southwest Asia on the Persian Gulf, bordering Oman and Saudi Arabia. The seven states, termed emirates, are Abu Dhabi, Ajman, Dubai, Fujairah, Ras al-Khaimah, Sharjah, and Umm al-Quwain.</obo:IAO_0000115>
        <oboInOwl:hasOBONamespace>GAZ</oboInOwl:hasOBONamespace>
        <oboInOwl:id>GAZ:00005282</oboInOwl:id>
        <rdfs:label>United Arab Emirates</rdfs:label>
    </owl:NamedIndividual>
    


    <!-- http://purl.obolibrary.org/obo/GAZ_00005287 -->

    <owl:NamedIndividual rdf:about="http://purl.obolibrary.org/obo/GAZ_00005287">
        <obo:RO_0001025 rdf:resource="http://purl.obolibrary.org/obo/GAZ_00005282"/>
    </owl:NamedIndividual>
    


    <!-- http://purl.obolibrary.org/obo/GAZ_00005288 -->

    <owl:NamedIndividual rdf:about="http://purl.obolibrary.org/obo/GAZ_00005288"/>
    


    <!-- http://purl.obolibrary.org/obo/GAZ_00005289 -->

    <owl:NamedIndividual rdf:about="http://purl.obolibrary.org/obo/GAZ_00005289"/>
    


    <!-- http://purl.obolibrary.org/obo/GAZ_00005290 -->

    <owl:NamedIndividual rdf:about="http://purl.obolibrary.org/obo/GAZ_00005290"/>
    


    <!-- http://purl.obolibrary.org/obo/GAZ_00005291 -->

    <owl:NamedIndividual rdf:about="http://purl.obolibrary.org/obo/GAZ_00005291"/>
    


    <!-- http://purl.obolibrary.org/obo/GAZ_00005292 -->

    <owl:NamedIndividual rdf:about="http://purl.obolibrary.org/obo/GAZ_00005292"/>
    


    <!-- http://purl.obolibrary.org/obo/GAZ_00005293 -->

    <owl:NamedIndividual rdf:about="http://purl.obolibrary.org/obo/GAZ_00005293"/>
    


    <!-- http://purl.obolibrary.org/obo/GAZ_00005294 -->

    <owl:NamedIndividual rdf:about="http://purl.obolibrary.org/obo/GAZ_00005294"/>
    


    <!-- http://purl.obolibrary.org/obo/GAZ_00008963 -->

    <owl:NamedIndividual rdf:about="http://purl.obolibrary.org/obo/GAZ_00008963">
        <obo:IAO_0000115>A wide strait linking the Persian Gulf and the Arabian Sea, are the following: On the North: A line joining Cape L Degrees mah (25 Degrees 56 Minutes 35 Seconds N - 56 Degrees 27 Minutes 30 Seconds E), in Oman, eastward to Cape Al K Degrees h (25 Degrees 47 Minutes 30 Seconds N - 57 Degrees 18 Minutes E), in Iran (the common limit with the Persian Gulf) and thence from Cape Al K Degrees h, in Iran, eastward, along the coasts of Iran and Pakistan, to Cape J Degrees wani (25 Degrees 01 Minutes 10 Seconds N -61 Degrees 44 Minutes 15 Seconds E), in Pakistan. On the East: A line joining Cape J Degrees wani, in Pakistan, southwestward to Cape Al H,add (22 Degrees 32 Minutes N - 59 Degrees 47 Minutes 30 Seconds E), in Oman (the common limit with the Arabian Sea). On the South and the West: From Cape Al H,add, in Oman, northwestward, along the coasts of Oman and the United Arab Emirates, to Cape L Degrees mah (25 Degrees 56 Minutes 35 Seconds N - 56 Degrees 27 Minutes 30 Seconds E), in Oman.</obo:IAO_0000115>
        <oboInOwl:hasOBONamespace>GAZ</oboInOwl:hasOBONamespace>
        <oboInOwl:id>GAZ:00008963</oboInOwl:id>
        <rdfs:label>Gulf of Oman</rdfs:label>
    </owl:NamedIndividual>
    


    <!-- http://purl.obolibrary.org/obo/GAZ_00047079 -->

    <owl:NamedIndividual rdf:about="http://purl.obolibrary.org/obo/GAZ_00047079">
        <obo:RO_0001025 rdf:resource="http://purl.obolibrary.org/obo/GAZ_00005291"/>
        <obo:IAO_0000115>An offshore Island in the Persian Gulf.</obo:IAO_0000115>
        <oboInOwl:hasOBONamespace>GAZ</oboInOwl:hasOBONamespace>
        <oboInOwl:id>GAZ:00047079</oboInOwl:id>
        <rdfs:label>Das</rdfs:label>
    </owl:NamedIndividual>
    


    <!-- http://purl.obolibrary.org/obo/GAZ_00047080 -->

    <owl:NamedIndividual rdf:about="http://purl.obolibrary.org/obo/GAZ_00047080">
        <obo:RO_0001025 rdf:resource="http://purl.obolibrary.org/obo/GAZ_00005291"/>
        <obo:IAO_0000115>An island off the coast of Abu Dhabi, United Arab Emirates.</obo:IAO_0000115>
        <oboInOwl:hasOBONamespace>GAZ</oboInOwl:hasOBONamespace>
        <oboInOwl:id>GAZ:00047080</oboInOwl:id>
        <rdfs:label>Dalma Island</rdfs:label>
    </owl:NamedIndividual>
    


    <!-- http://purl.obolibrary.org/obo/GAZ_00047081 -->

    <owl:NamedIndividual rdf:about="http://purl.obolibrary.org/obo/GAZ_00047081">
        <obo:RO_0001025 rdf:resource="http://purl.obolibrary.org/obo/GAZ_00005291"/>
        <obo:IAO_0000115>An island.</obo:IAO_0000115>
        <oboInOwl:hasOBONamespace>GAZ</oboInOwl:hasOBONamespace>
        <oboInOwl:id>GAZ:00047081</oboInOwl:id>
        <rdfs:label>Arzanah Island</rdfs:label>
    </owl:NamedIndividual>
    


    <!-- http://purl.obolibrary.org/obo/GAZ_00048832 -->

    <owl:NamedIndividual rdf:about="http://purl.obolibrary.org/obo/GAZ_00048832">
        <obo:RO_0001025 rdf:resource="http://purl.obolibrary.org/obo/GAZ_00008963"/>
        <obo:IAO_0000115>An island off the East coast of Oman.</obo:IAO_0000115>
        <oboInOwl:hasOBONamespace>GAZ</oboInOwl:hasOBONamespace>
        <oboInOwl:id>GAZ:00048832</oboInOwl:id>
        <rdfs:label>Masirah Island</rdfs:label>
    </owl:NamedIndividual>
    


    <!-- http://purl.obolibrary.org/obo/GAZ_00049020 -->

    <owl:NamedIndividual rdf:about="http://purl.obolibrary.org/obo/GAZ_00049020">
        <obo:RO_0001025 rdf:resource="http://purl.obolibrary.org/obo/GAZ_00005291"/>
        <obo:IAO_0000115>The largest of about 200 islands along the coast of the United Arab Emirates. It is situated in the emirate of Abu Dhabi.</obo:IAO_0000115>
        <oboInOwl:hasOBONamespace>GAZ</oboInOwl:hasOBONamespace>
        <oboInOwl:id>GAZ:00049020</oboInOwl:id>
        <rdfs:label>Abu al Abyad</rdfs:label>
    </owl:NamedIndividual>
    


    <!-- http://purl.obolibrary.org/obo/GAZ_00051769 -->

    <owl:NamedIndividual rdf:about="http://purl.obolibrary.org/obo/GAZ_00051769">
        <obo:RO_0001025 rdf:resource="http://purl.obolibrary.org/obo/GAZ_00005289"/>
        <obo:IAO_0000115>An archipelago of artificial islands off the coast of Dubai.</obo:IAO_0000115>
        <oboInOwl:hasOBONamespace>GAZ</oboInOwl:hasOBONamespace>
        <oboInOwl:id>GAZ:00051769</oboInOwl:id>
        <rdfs:label>OQYANA</rdfs:label>
    </owl:NamedIndividual>
    


    <!-- http://purl.obolibrary.org/obo/GAZ_00052016 -->

    <owl:NamedIndividual rdf:about="http://purl.obolibrary.org/obo/GAZ_00052016">
        <obo:RO_0001025 rdf:resource="http://purl.obolibrary.org/obo/GAZ_00005288"/>
        <obo:IAO_0000115>One of the villages of Dibba, ruled by the Emirate of Fujairah.</obo:IAO_0000115>
        <oboInOwl:hasOBONamespace>GAZ</oboInOwl:hasOBONamespace>
        <oboInOwl:id>GAZ:00052016</oboInOwl:id>
        <rdfs:label>Dibba Al Fujairah</rdfs:label>
    </owl:NamedIndividual>
    


    <!-- http://purl.obolibrary.org/obo/GAZ_00052017 -->

    <owl:NamedIndividual rdf:about="http://purl.obolibrary.org/obo/GAZ_00052017">
        <obo:RO_0001025 rdf:resource="http://purl.obolibrary.org/obo/GAZ_00005294"/>
        <obo:IAO_0000115>One of the villages of Dibba, ruled by the Emirate of Sharjah.</obo:IAO_0000115>
        <oboInOwl:hasOBONamespace>GAZ</oboInOwl:hasOBONamespace>
        <oboInOwl:id>GAZ:00052017</oboInOwl:id>
        <rdfs:label>Hisn Dibba</rdfs:label>
    </owl:NamedIndividual>
    


    <!-- http://purl.obolibrary.org/obo/GAZ_00053001 -->

    <owl:NamedIndividual rdf:about="http://purl.obolibrary.org/obo/GAZ_00053001">
        <obo:IAO_0000115>A mountain located in northeastern Oman. It is the highest mountain of the country.</obo:IAO_0000115>
        <oboInOwl:hasOBONamespace>GAZ</oboInOwl:hasOBONamespace>
        <oboInOwl:id>GAZ:00053001</oboInOwl:id>
        <rdfs:label>Jebel Shams</rdfs:label>
    </owl:NamedIndividual>
    


    <!-- http://purl.obolibrary.org/obo/GAZ_00057451 -->

    <owl:NamedIndividual rdf:about="http://purl.obolibrary.org/obo/GAZ_00057451">
        <obo:IAO_0000115>A part of the Al Hajar Mountains range in Oman, which extends about 300 km northwest to southeast, between 50-100 km inland from the Gulf of Oman coast. It comprises the central section of the Al Hajar Mountains range, and is located around 150 km from Muscat.</obo:IAO_0000115>
        <oboInOwl:hasOBONamespace>GAZ</oboInOwl:hasOBONamespace>
        <oboInOwl:id>GAZ:00057451</oboInOwl:id>
        <rdfs:label>Jebel Akhdar</rdfs:label>
    </owl:NamedIndividual>
    


    <!-- http://purl.obolibrary.org/obo/GAZ_00078570 -->

    <owl:NamedIndividual rdf:about="http://purl.obolibrary.org/obo/GAZ_00078570">
        <obo:RO_0001025 rdf:resource="http://purl.obolibrary.org/obo/GAZ_00005291"/>
        <obo:IAO_0000115>The fourth largest city in the United Arab Emirates (UAE). It is located in Abu Dhabi (emirate), directly adjacent to the border with Oman.</obo:IAO_0000115>
        <oboInOwl:hasOBONamespace>GAZ</oboInOwl:hasOBONamespace>
        <oboInOwl:id>GAZ:00078570</oboInOwl:id>
        <rdfs:label>Al Ain</rdfs:label>
    </owl:NamedIndividual>
    


    <!-- http://purl.obolibrary.org/obo/GAZ_00078571 -->

    <owl:NamedIndividual rdf:about="http://purl.obolibrary.org/obo/GAZ_00078571">
        <rdf:type rdf:resource="http://purl.obolibrary.org/obo/ENVO_00000856"/>
        <obo:RO_0001025 rdf:resource="http://purl.obolibrary.org/obo/GAZ_00005291"/>
        <obo:IAO_0000115>A populated place. A town in the Emirate of Abu Dhabi.</obo:IAO_0000115>
        <oboInOwl:hasOBONamespace>GAZ</oboInOwl:hasOBONamespace>
        <oboInOwl:id>GAZ:00078571</oboInOwl:id>
        <rdfs:label>Baniyas</rdfs:label>
    </owl:NamedIndividual>
    


    <!-- http://purl.obolibrary.org/obo/GAZ_00078572 -->

    <owl:NamedIndividual rdf:about="http://purl.obolibrary.org/obo/GAZ_00078572">
        <rdf:type rdf:resource="http://purl.obolibrary.org/obo/ENVO_00000856"/>
        <obo:RO_0001025 rdf:resource="http://purl.obolibrary.org/obo/GAZ_00005291"/>
        <obo:IAO_0000115>A populated place. A town located some 240 km west of Abu Dhabi city.</obo:IAO_0000115>
        <oboInOwl:hasOBONamespace>GAZ</oboInOwl:hasOBONamespace>
        <oboInOwl:id>GAZ:00078572</oboInOwl:id>
        <rdfs:label>Ruwais</rdfs:label>
    </owl:NamedIndividual>
    


    <!-- http://purl.obolibrary.org/obo/GAZ_00078574 -->

    <owl:NamedIndividual rdf:about="http://purl.obolibrary.org/obo/GAZ_00078574">
        <obo:RO_0001025 rdf:resource="http://purl.obolibrary.org/obo/GAZ_00005291"/>
        <obo:IAO_0000115>A natural island 600 m off the coast of Abu Dhabi island.</obo:IAO_0000115>
        <oboInOwl:hasOBONamespace>GAZ</oboInOwl:hasOBONamespace>
        <oboInOwl:id>GAZ:00078574</oboInOwl:id>
        <rdfs:label>Al Reem Island</rdfs:label>
    </owl:NamedIndividual>
    


    <!-- http://purl.obolibrary.org/obo/GAZ_00078575 -->

    <owl:NamedIndividual rdf:about="http://purl.obolibrary.org/obo/GAZ_00078575">
        <obo:RO_0001025 rdf:resource="http://purl.obolibrary.org/obo/GAZ_00005291"/>
        <obo:IAO_0000115>A large, low lying island 500 m off the coast of Abu Dhabi island.</obo:IAO_0000115>
        <oboInOwl:hasOBONamespace>GAZ</oboInOwl:hasOBONamespace>
        <oboInOwl:id>GAZ:00078575</oboInOwl:id>
        <rdfs:label>Saadiyat Island</rdfs:label>
    </owl:NamedIndividual>
    


    <!-- http://purl.obolibrary.org/obo/GAZ_00078576 -->

    <owl:NamedIndividual rdf:about="http://purl.obolibrary.org/obo/GAZ_00078576">
        <obo:RO_0001025 rdf:resource="http://purl.obolibrary.org/obo/GAZ_00005291"/>
        <oboInOwl:hasOBONamespace>GAZ</oboInOwl:hasOBONamespace>
        <oboInOwl:id>GAZ:00078576</oboInOwl:id>
        <rdfs:label>Abu Dhabi Island</rdfs:label>
    </owl:NamedIndividual>
    


    <!-- http://purl.obolibrary.org/obo/GAZ_00078577 -->

    <owl:NamedIndividual rdf:about="http://purl.obolibrary.org/obo/GAZ_00078577">
        <obo:RO_0001025 rdf:resource="http://purl.obolibrary.org/obo/GAZ_00005290"/>
        <obo:IAO_0000115>The capital of the emirate of Ajman located along the Persian Gulf.</obo:IAO_0000115>
        <oboInOwl:hasOBONamespace>GAZ</oboInOwl:hasOBONamespace>
        <oboInOwl:id>GAZ:00078577</oboInOwl:id>
        <rdfs:label>Ajman</rdfs:label>
    </owl:NamedIndividual>
    


    <!-- http://purl.obolibrary.org/obo/GAZ_00078578 -->

    <owl:NamedIndividual rdf:about="http://purl.obolibrary.org/obo/GAZ_00078578">
        <obo:RO_0001025 rdf:resource="http://purl.obolibrary.org/obo/GAZ_00005290"/>
        <obo:IAO_0000115>A populated place. A city in Ajman.</obo:IAO_0000115>
        <oboInOwl:hasOBONamespace>GAZ</oboInOwl:hasOBONamespace>
        <oboInOwl:id>GAZ:00078578</oboInOwl:id>
        <rdfs:label>Masfut</rdfs:label>
    </owl:NamedIndividual>
    


    <!-- http://purl.obolibrary.org/obo/GAZ_00078579 -->

    <owl:NamedIndividual rdf:about="http://purl.obolibrary.org/obo/GAZ_00078579">
        <obo:RO_0001025 rdf:resource="http://purl.obolibrary.org/obo/GAZ_00005289"/>
        <obo:IAO_0000115>A city.</obo:IAO_0000115>
        <oboInOwl:hasOBONamespace>GAZ</oboInOwl:hasOBONamespace>
        <oboInOwl:id>GAZ:00078579</oboInOwl:id>
        <rdfs:label>Dubai</rdfs:label>
    </owl:NamedIndividual>
    


    <!-- http://purl.obolibrary.org/obo/GAZ_00078580 -->

    <owl:NamedIndividual rdf:about="http://purl.obolibrary.org/obo/GAZ_00078580">
        <rdf:type rdf:resource="http://purl.obolibrary.org/obo/ENVO_00000856"/>
        <obo:RO_0001025 rdf:resource="http://purl.obolibrary.org/obo/GAZ_00005289"/>
        <obo:IAO_0000115>A populated place. A town in the Hatta mountains in the north of the emirate of Dubai.</obo:IAO_0000115>
        <oboInOwl:hasOBONamespace>GAZ</oboInOwl:hasOBONamespace>
        <oboInOwl:id>GAZ:00078580</oboInOwl:id>
        <rdfs:label>Hatta</rdfs:label>
    </owl:NamedIndividual>
    


    <!-- http://purl.obolibrary.org/obo/GAZ_00078581 -->

    <owl:NamedIndividual rdf:about="http://purl.obolibrary.org/obo/GAZ_00078581">
        <rdf:type rdf:resource="http://purl.obolibrary.org/obo/ENVO_00000856"/>
        <obo:RO_0001025 rdf:resource="http://purl.obolibrary.org/obo/GAZ_00005294"/>
        <obo:IAO_0000115>A populated place. A town in the emirate of Sharjah in the United Arab Emirates (UAE). Located along the Gulf of Oman, Khor Fakkan is geographically surrounded by the emirate of Fujairah.</obo:IAO_0000115>
        <oboInOwl:hasOBONamespace>GAZ</oboInOwl:hasOBONamespace>
        <oboInOwl:id>GAZ:00078581</oboInOwl:id>
        <rdfs:label>Khor Fakkan</rdfs:label>
    </owl:NamedIndividual>
    


    <!-- http://purl.obolibrary.org/obo/GAZ_00078582 -->

    <owl:NamedIndividual rdf:about="http://purl.obolibrary.org/obo/GAZ_00078582">
        <rdf:type rdf:resource="http://purl.obolibrary.org/obo/ENVO_00000856"/>
        <obo:RO_0001025 rdf:resource="http://purl.obolibrary.org/obo/GAZ_00005294"/>
        <obo:IAO_0000115>A populated place. A town in the United Arab Emirates. Politically part of the emirate of Sharjah, Kalba is the south by Oman and in the north by the emirate of Fujairah.</obo:IAO_0000115>
        <oboInOwl:hasOBONamespace>GAZ</oboInOwl:hasOBONamespace>
        <oboInOwl:id>GAZ:00078582</oboInOwl:id>
        <rdfs:label>Kalba</rdfs:label>
    </owl:NamedIndividual>
    


    <!-- http://purl.obolibrary.org/obo/GAZ_00078583 -->

    <owl:NamedIndividual rdf:about="http://purl.obolibrary.org/obo/GAZ_00078583">
        <obo:RO_0001025 rdf:resource="http://purl.obolibrary.org/obo/GAZ_00078582"/>
        <obo:IAO_0000115>A mangrove island S of Kalba.</obo:IAO_0000115>
        <oboInOwl:hasOBONamespace>GAZ</oboInOwl:hasOBONamespace>
        <oboInOwl:id>GAZ:00078583</oboInOwl:id>
        <rdfs:label>Khor Kalba</rdfs:label>
    </owl:NamedIndividual>
    


    <!-- http://purl.obolibrary.org/obo/GAZ_00078584 -->

    <owl:NamedIndividual rdf:about="http://purl.obolibrary.org/obo/GAZ_00078584">
        <rdf:type rdf:resource="http://purl.obolibrary.org/obo/ENVO_00000856"/>
        <obo:RO_0001025 rdf:resource="http://purl.obolibrary.org/obo/GAZ_00005288"/>
        <obo:RO_0001025 rdf:resource="http://purl.obolibrary.org/obo/GAZ_00005293"/>
        <obo:IAO_0000115>A populated place. A village located on the edge of the Hajar Mountains in the United Arab Emirates. The village is divided into two parts: the larger belongs to the Emirate of Ras al-Khaimah, the smaller belongs to the emirate of Fujairah.</obo:IAO_0000115>
        <oboInOwl:hasOBONamespace>GAZ</oboInOwl:hasOBONamespace>
        <oboInOwl:id>GAZ:00078584</oboInOwl:id>
        <rdfs:label>Masafi</rdfs:label>
    </owl:NamedIndividual>
    


    <!-- http://purl.obolibrary.org/obo/GAZ_00078585 -->

    <owl:NamedIndividual rdf:about="http://purl.obolibrary.org/obo/GAZ_00078585">
        <obo:RO_0001025 rdf:resource="http://purl.obolibrary.org/obo/GAZ_00005294"/>
        <obo:IAO_0000115>The third most populous city in the United Arab Emirates and is the seat of government of the emirate of Sharjah.</obo:IAO_0000115>
        <oboInOwl:hasOBONamespace>GAZ</oboInOwl:hasOBONamespace>
        <oboInOwl:id>GAZ:00078585</oboInOwl:id>
        <rdfs:label>Sharjah</rdfs:label>
    </owl:NamedIndividual>
    


    <!-- http://purl.obolibrary.org/obo/GAZ_00145498 -->

    <owl:NamedIndividual rdf:about="http://purl.obolibrary.org/obo/GAZ_00145498">
        <obo:RO_0001025 rdf:resource="http://purl.obolibrary.org/obo/GAZ_00005289"/>
        <obo:IAO_0000115>A saltwater creek located in Dubai, United Arab Emirates.</obo:IAO_0000115>
        <oboInOwl:hasOBONamespace>GAZ</oboInOwl:hasOBONamespace>
        <oboInOwl:id>GAZ:00145498</oboInOwl:id>
        <rdfs:label>Dubai Creek</rdfs:label>
    </owl:NamedIndividual>
    


    <!-- http://purl.obolibrary.org/obo/GAZ_00145499 -->

    <owl:NamedIndividual rdf:about="http://purl.obolibrary.org/obo/GAZ_00145499">
        <obo:RO_0001025 rdf:resource="http://purl.obolibrary.org/obo/GAZ_00005289"/>
        <obo:IAO_0000115>A tidal inlet. Includes a wetland reserve in the Emirate of Dubai.</obo:IAO_0000115>
        <oboInOwl:hasOBONamespace>GAZ</oboInOwl:hasOBONamespace>
        <oboInOwl:id>GAZ:00145499</oboInOwl:id>
        <rdfs:label>Ras Al Khor</rdfs:label>
    </owl:NamedIndividual>
    


    <!-- http://purl.obolibrary.org/obo/GAZ_00147025 -->

    <owl:NamedIndividual rdf:about="http://purl.obolibrary.org/obo/GAZ_00147025">
        <obo:RO_0001025 rdf:resource="http://purl.obolibrary.org/obo/GAZ_00005288"/>
        <obo:RO_0001025 rdf:resource="http://purl.obolibrary.org/obo/GAZ_00008963"/>
        <obo:IAO_0000115>A cove in Fujairah.</obo:IAO_0000115>
        <oboInOwl:hasOBONamespace>GAZ</oboInOwl:hasOBONamespace>
        <oboInOwl:id>GAZ:00147025</oboInOwl:id>
        <rdfs:label>Ad Dayt</rdfs:label>
    </owl:NamedIndividual>
    


    <!-- http://purl.obolibrary.org/obo/GAZ_00248023 -->

    <owl:NamedIndividual rdf:about="http://purl.obolibrary.org/obo/GAZ_00248023">
        <obo:RO_0001025 rdf:resource="http://purl.obolibrary.org/obo/GAZ_00005291"/>
        <obo:IAO_0000115>An island.</obo:IAO_0000115>
        <oboInOwl:hasOBONamespace>GAZ</oboInOwl:hasOBONamespace>
        <oboInOwl:id>GAZ:00248023</oboInOwl:id>
        <rdfs:label>Sir Bani Yas</rdfs:label>
    </owl:NamedIndividual>
    


    <!-- http://purl.obolibrary.org/obo/GAZ_00248024 -->

    <owl:NamedIndividual rdf:about="http://purl.obolibrary.org/obo/GAZ_00248024">
        <obo:RO_0001025 rdf:resource="http://purl.obolibrary.org/obo/GAZ_00005291"/>
        <obo:IAO_0000115>A channel.</obo:IAO_0000115>
        <oboInOwl:hasOBONamespace>GAZ</oboInOwl:hasOBONamespace>
        <oboInOwl:id>GAZ:00248024</oboInOwl:id>
        <rdfs:label>Khawr al Bazm</rdfs:label>
    </owl:NamedIndividual>
    


    <!-- http://purl.obolibrary.org/obo/GAZ_00248025 -->

    <owl:NamedIndividual rdf:about="http://purl.obolibrary.org/obo/GAZ_00248025">
        <obo:RO_0001025 rdf:resource="http://purl.obolibrary.org/obo/GAZ_00005291"/>
        <obo:IAO_0000115>An island.</obo:IAO_0000115>
        <oboInOwl:hasOBONamespace>GAZ</oboInOwl:hasOBONamespace>
        <oboInOwl:id>GAZ:00248025</oboInOwl:id>
        <rdfs:label>Bu Khushayshah</rdfs:label>
    </owl:NamedIndividual>
    


    <!-- http://purl.obolibrary.org/obo/GAZ_00248026 -->

    <owl:NamedIndividual rdf:about="http://purl.obolibrary.org/obo/GAZ_00248026">
        <obo:RO_0001025 rdf:resource="http://purl.obolibrary.org/obo/GAZ_00005291"/>
        <obo:IAO_0000115>An island.</obo:IAO_0000115>
        <oboInOwl:hasOBONamespace>GAZ</oboInOwl:hasOBONamespace>
        <oboInOwl:id>GAZ:00248026</oboInOwl:id>
        <rdfs:label>Al Futaysi</rdfs:label>
    </owl:NamedIndividual>
    


    <!-- http://purl.obolibrary.org/obo/GAZ_00248027 -->

    <owl:NamedIndividual rdf:about="http://purl.obolibrary.org/obo/GAZ_00248027">
        <obo:RO_0001025 rdf:resource="http://purl.obolibrary.org/obo/GAZ_00005291"/>
        <obo:IAO_0000115>An island.</obo:IAO_0000115>
        <oboInOwl:hasOBONamespace>GAZ</oboInOwl:hasOBONamespace>
        <oboInOwl:id>GAZ:00248027</oboInOwl:id>
        <rdfs:label>Halat al Bahrani</rdfs:label>
    </owl:NamedIndividual>
    


    <!-- http://purl.obolibrary.org/obo/GAZ_00248028 -->

    <owl:NamedIndividual rdf:about="http://purl.obolibrary.org/obo/GAZ_00248028">
        <obo:RO_0001025 rdf:resource="http://purl.obolibrary.org/obo/GAZ_00005291"/>
        <obo:IAO_0000115>An island.</obo:IAO_0000115>
        <oboInOwl:hasOBONamespace>GAZ</oboInOwl:hasOBONamespace>
        <oboInOwl:id>GAZ:00248028</oboInOwl:id>
        <rdfs:label>&apos;Ushsh</rdfs:label>
    </owl:NamedIndividual>
    


    <!-- http://purl.obolibrary.org/obo/GAZ_00248029 -->

    <owl:NamedIndividual rdf:about="http://purl.obolibrary.org/obo/GAZ_00248029">
        <obo:RO_0001025 rdf:resource="http://purl.obolibrary.org/obo/GAZ_00005291"/>
        <obo:IAO_0000115>An island.</obo:IAO_0000115>
        <oboInOwl:hasOBONamespace>GAZ</oboInOwl:hasOBONamespace>
        <oboInOwl:id>GAZ:00248029</oboInOwl:id>
        <rdfs:label>Umm &apos;Amim</rdfs:label>
    </owl:NamedIndividual>
    


    <!-- http://purl.obolibrary.org/obo/GAZ_00248030 -->

    <owl:NamedIndividual rdf:about="http://purl.obolibrary.org/obo/GAZ_00248030">
        <obo:RO_0001025 rdf:resource="http://purl.obolibrary.org/obo/GAZ_00005291"/>
        <obo:IAO_0000115>An island.</obo:IAO_0000115>
        <oboInOwl:hasOBONamespace>GAZ</oboInOwl:hasOBONamespace>
        <oboInOwl:id>GAZ:00248030</oboInOwl:id>
        <rdfs:label>Jananah</rdfs:label>
    </owl:NamedIndividual>
    


    <!-- http://purl.obolibrary.org/obo/GAZ_00248031 -->

    <owl:NamedIndividual rdf:about="http://purl.obolibrary.org/obo/GAZ_00248031">
        <rdf:type rdf:resource="http://purl.obolibrary.org/obo/ENVO_00000167"/>
        <obo:RO_0001025 rdf:resource="http://purl.obolibrary.org/obo/GAZ_00005291"/>
        <obo:IAO_0000115>A shoal.</obo:IAO_0000115>
        <oboInOwl:hasOBONamespace>GAZ</oboInOwl:hasOBONamespace>
        <oboInOwl:id>GAZ:00248031</oboInOwl:id>
        <rdfs:label>Bu Tinah</rdfs:label>
    </owl:NamedIndividual>
    


    <!-- http://purl.obolibrary.org/obo/GAZ_00248032 -->

    <owl:NamedIndividual rdf:about="http://purl.obolibrary.org/obo/GAZ_00248032">
        <obo:RO_0001025 rdf:resource="http://purl.obolibrary.org/obo/GAZ_00005291"/>
        <obo:IAO_0000115>An island.</obo:IAO_0000115>
        <oboInOwl:hasOBONamespace>GAZ</oboInOwl:hasOBONamespace>
        <oboInOwl:id>GAZ:00248032</oboInOwl:id>
        <rdfs:label>Salahah</rdfs:label>
    </owl:NamedIndividual>
    


    <!-- http://purl.obolibrary.org/obo/GAZ_00248033 -->

    <owl:NamedIndividual rdf:about="http://purl.obolibrary.org/obo/GAZ_00248033">
        <obo:RO_0001025 rdf:resource="http://purl.obolibrary.org/obo/GAZ_00005291"/>
        <obo:IAO_0000115>An island.</obo:IAO_0000115>
        <oboInOwl:hasOBONamespace>GAZ</oboInOwl:hasOBONamespace>
        <oboInOwl:id>GAZ:00248033</oboInOwl:id>
        <rdfs:label>Jazirat Marawwah</rdfs:label>
    </owl:NamedIndividual>
    


    <!-- http://purl.obolibrary.org/obo/GAZ_00248034 -->

    <owl:NamedIndividual rdf:about="http://purl.obolibrary.org/obo/GAZ_00248034">
        <obo:RO_0001025 rdf:resource="http://purl.obolibrary.org/obo/GAZ_00005291"/>
        <obo:IAO_0000115>An island.</obo:IAO_0000115>
        <oboInOwl:hasOBONamespace>GAZ</oboInOwl:hasOBONamespace>
        <oboInOwl:id>GAZ:00248034</oboInOwl:id>
        <rdfs:label>Al Bazm al Gharbica</rdfs:label>
    </owl:NamedIndividual>
    


    <!-- http://purl.obolibrary.org/obo/GAZ_00248035 -->

    <owl:NamedIndividual rdf:about="http://purl.obolibrary.org/obo/GAZ_00248035">
        <obo:RO_0001025 rdf:resource="http://purl.obolibrary.org/obo/GAZ_00005291"/>
        <obo:IAO_0000115>An island. A satellite of Sir Bani Yas.</obo:IAO_0000115>
        <oboInOwl:hasOBONamespace>GAZ</oboInOwl:hasOBONamespace>
        <oboInOwl:id>GAZ:00248035</oboInOwl:id>
        <rdfs:label>Umm Qassar</rdfs:label>
    </owl:NamedIndividual>
    


    <!-- http://purl.obolibrary.org/obo/GAZ_00248036 -->

    <owl:NamedIndividual rdf:about="http://purl.obolibrary.org/obo/GAZ_00248036">
        <obo:RO_0001025 rdf:resource="http://purl.obolibrary.org/obo/GAZ_00005291"/>
        <oboInOwl:hasOBONamespace>GAZ</oboInOwl:hasOBONamespace>
        <oboInOwl:id>GAZ:00248036</oboInOwl:id>
        <rdfs:label>Umm al Kirkum</rdfs:label>
    </owl:NamedIndividual>
    


    <!-- http://purl.obolibrary.org/obo/GAZ_00248037 -->

    <owl:NamedIndividual rdf:about="http://purl.obolibrary.org/obo/GAZ_00248037">
        <obo:RO_0001025 rdf:resource="http://purl.obolibrary.org/obo/GAZ_00005291"/>
        <oboInOwl:hasOBONamespace>GAZ</oboInOwl:hasOBONamespace>
        <oboInOwl:id>GAZ:00248037</oboInOwl:id>
        <rdfs:label>Ghasha</rdfs:label>
    </owl:NamedIndividual>
    


    <!-- http://purl.obolibrary.org/obo/GAZ_00248038 -->

    <owl:NamedIndividual rdf:about="http://purl.obolibrary.org/obo/GAZ_00248038">
        <obo:RO_0001025 rdf:resource="http://purl.obolibrary.org/obo/GAZ_00005291"/>
        <obo:IAO_0000115>An island.</obo:IAO_0000115>
        <oboInOwl:hasOBONamespace>GAZ</oboInOwl:hasOBONamespace>
        <oboInOwl:id>GAZ:00248038</oboInOwl:id>
        <rdfs:label>Al Yasat</rdfs:label>
    </owl:NamedIndividual>
    


    <!-- http://purl.obolibrary.org/obo/GAZ_00248039 -->

    <owl:NamedIndividual rdf:about="http://purl.obolibrary.org/obo/GAZ_00248039">
        <obo:RO_0001025 rdf:resource="http://purl.obolibrary.org/obo/GAZ_00005291"/>
        <obo:IAO_0000115>An island.</obo:IAO_0000115>
        <oboInOwl:hasOBONamespace>GAZ</oboInOwl:hasOBONamespace>
        <oboInOwl:id>GAZ:00248039</oboInOwl:id>
        <rdfs:label>Al Yasat as Sufla</rdfs:label>
    </owl:NamedIndividual>
    


    <!-- http://purl.obolibrary.org/obo/GAZ_00248040 -->

    <owl:NamedIndividual rdf:about="http://purl.obolibrary.org/obo/GAZ_00248040">
        <obo:RO_0001025 rdf:resource="http://purl.obolibrary.org/obo/GAZ_00005291"/>
        <obo:IAO_0000115>An island.</obo:IAO_0000115>
        <oboInOwl:hasOBONamespace>GAZ</oboInOwl:hasOBONamespace>
        <oboInOwl:id>GAZ:00248040</oboInOwl:id>
        <rdfs:label>Al Yasat al &apos;Ulya</rdfs:label>
    </owl:NamedIndividual>
    


    <!-- http://purl.obolibrary.org/obo/GAZ_00248041 -->

    <owl:NamedIndividual rdf:about="http://purl.obolibrary.org/obo/GAZ_00248041">
        <obo:RO_0001025 rdf:resource="http://purl.obolibrary.org/obo/GAZ_00005291"/>
        <obo:IAO_0000115>An island.</obo:IAO_0000115>
        <oboInOwl:hasOBONamespace>GAZ</oboInOwl:hasOBONamespace>
        <oboInOwl:id>GAZ:00248041</oboInOwl:id>
        <rdfs:label>Ghaghah</rdfs:label>
    </owl:NamedIndividual>
    


    <!-- http://purl.obolibrary.org/obo/GAZ_00248042 -->

    <owl:NamedIndividual rdf:about="http://purl.obolibrary.org/obo/GAZ_00248042">
        <obo:RO_0001025 rdf:resource="http://purl.obolibrary.org/obo/GAZ_00005291"/>
        <obo:IAO_0000115>An island.</obo:IAO_0000115>
        <oboInOwl:hasOBONamespace>GAZ</oboInOwl:hasOBONamespace>
        <oboInOwl:id>GAZ:00248042</oboInOwl:id>
        <rdfs:label>Umm al Hatab</rdfs:label>
    </owl:NamedIndividual>
    


    <!-- http://purl.obolibrary.org/obo/GAZ_00248043 -->

    <owl:NamedIndividual rdf:about="http://purl.obolibrary.org/obo/GAZ_00248043">
        <obo:RO_0001025 rdf:resource="http://purl.obolibrary.org/obo/GAZ_00005291"/>
        <obo:IAO_0000115>An island.</obo:IAO_0000115>
        <oboInOwl:hasOBONamespace>GAZ</oboInOwl:hasOBONamespace>
        <oboInOwl:id>GAZ:00248043</oboInOwl:id>
        <rdfs:label>Makasib</rdfs:label>
    </owl:NamedIndividual>
    


    <!-- http://purl.obolibrary.org/obo/GAZ_00248044 -->

    <owl:NamedIndividual rdf:about="http://purl.obolibrary.org/obo/GAZ_00248044">
        <obo:RO_0001025 rdf:resource="http://purl.obolibrary.org/obo/GAZ_00005291"/>
        <obo:IAO_0000115>An island.</obo:IAO_0000115>
        <oboInOwl:hasOBONamespace>GAZ</oboInOwl:hasOBONamespace>
        <oboInOwl:id>GAZ:00248044</oboInOwl:id>
        <rdfs:label>Al Qaffay</rdfs:label>
    </owl:NamedIndividual>
    


    <!-- http://purl.obolibrary.org/obo/GAZ_00248045 -->

    <owl:NamedIndividual rdf:about="http://purl.obolibrary.org/obo/GAZ_00248045">
        <obo:RO_0001025 rdf:resource="http://purl.obolibrary.org/obo/GAZ_00005291"/>
        <obo:IAO_0000115>An island.</obo:IAO_0000115>
        <oboInOwl:hasOBONamespace>GAZ</oboInOwl:hasOBONamespace>
        <oboInOwl:id>GAZ:00248045</oboInOwl:id>
        <rdfs:label>Muhammaliyah</rdfs:label>
    </owl:NamedIndividual>
    


    <!-- http://purl.obolibrary.org/obo/GAZ_00248046 -->

    <owl:NamedIndividual rdf:about="http://purl.obolibrary.org/obo/GAZ_00248046">
        <obo:RO_0001025 rdf:resource="http://purl.obolibrary.org/obo/GAZ_00005291"/>
        <obo:IAO_0000115>An offshore island.</obo:IAO_0000115>
        <oboInOwl:hasOBONamespace>GAZ</oboInOwl:hasOBONamespace>
        <oboInOwl:id>GAZ:00248046</oboInOwl:id>
        <rdfs:label>Dayyinah</rdfs:label>
    </owl:NamedIndividual>
    


    <!-- http://purl.obolibrary.org/obo/GAZ_00248047 -->

    <owl:NamedIndividual rdf:about="http://purl.obolibrary.org/obo/GAZ_00248047">
        <obo:RO_0001025 rdf:resource="http://purl.obolibrary.org/obo/GAZ_00005291"/>
        <obo:IAO_0000115>An offshore island.</obo:IAO_0000115>
        <oboInOwl:hasOBONamespace>GAZ</oboInOwl:hasOBONamespace>
        <oboInOwl:id>GAZ:00248047</oboInOwl:id>
        <rdfs:label>Qarnayn</rdfs:label>
    </owl:NamedIndividual>
    


    <!-- http://purl.obolibrary.org/obo/GAZ_00248048 -->

    <owl:NamedIndividual rdf:about="http://purl.obolibrary.org/obo/GAZ_00248048">
        <obo:RO_0001025 rdf:resource="http://purl.obolibrary.org/obo/GAZ_00005291"/>
        <obo:IAO_0000115>An offshore island.</obo:IAO_0000115>
        <oboInOwl:hasOBONamespace>GAZ</oboInOwl:hasOBONamespace>
        <oboInOwl:id>GAZ:00248048</oboInOwl:id>
        <rdfs:label>Arzanah</rdfs:label>
    </owl:NamedIndividual>
    


    <!-- http://purl.obolibrary.org/obo/GAZ_00248049 -->

    <owl:NamedIndividual rdf:about="http://purl.obolibrary.org/obo/GAZ_00248049">
        <obo:RO_0001025 rdf:resource="http://purl.obolibrary.org/obo/GAZ_00005291"/>
        <obo:IAO_0000115>An offshore island.</obo:IAO_0000115>
        <oboInOwl:hasOBONamespace>GAZ</oboInOwl:hasOBONamespace>
        <oboInOwl:id>GAZ:00248049</oboInOwl:id>
        <rdfs:label>Zirkuh</rdfs:label>
    </owl:NamedIndividual>
    


    <!-- http://purl.obolibrary.org/obo/GAZ_00248050 -->

    <owl:NamedIndividual rdf:about="http://purl.obolibrary.org/obo/GAZ_00248050">
        <obo:RO_0001025 rdf:resource="http://purl.obolibrary.org/obo/GAZ_00005291"/>
        <obo:IAO_0000115>An island off eastern Abu Dhabi.</obo:IAO_0000115>
        <oboInOwl:hasOBONamespace>GAZ</oboInOwl:hasOBONamespace>
        <oboInOwl:id>GAZ:00248050</oboInOwl:id>
        <rdfs:label>As Sa&apos;diyat</rdfs:label>
    </owl:NamedIndividual>
    


    <!-- http://purl.obolibrary.org/obo/GAZ_00248051 -->

    <owl:NamedIndividual rdf:about="http://purl.obolibrary.org/obo/GAZ_00248051">
        <obo:RO_0001025 rdf:resource="http://purl.obolibrary.org/obo/GAZ_00005291"/>
        <obo:IAO_0000115>An island off eastern Abu Dhabi.</obo:IAO_0000115>
        <oboInOwl:hasOBONamespace>GAZ</oboInOwl:hasOBONamespace>
        <oboInOwl:id>GAZ:00248051</oboInOwl:id>
        <rdfs:label>Jazirat Ramhan</rdfs:label>
    </owl:NamedIndividual>
    


    <!-- http://purl.obolibrary.org/obo/GAZ_00248052 -->

    <owl:NamedIndividual rdf:about="http://purl.obolibrary.org/obo/GAZ_00248052">
        <obo:RO_0001025 rdf:resource="http://purl.obolibrary.org/obo/GAZ_00005291"/>
        <obo:IAO_0000115>An island off eastern Abu Dhabi.</obo:IAO_0000115>
        <oboInOwl:hasOBONamespace>GAZ</oboInOwl:hasOBONamespace>
        <oboInOwl:id>GAZ:00248052</oboInOwl:id>
        <rdfs:label>Bu Hayl</rdfs:label>
    </owl:NamedIndividual>
    


    <!-- http://purl.obolibrary.org/obo/GAZ_00248053 -->

    <owl:NamedIndividual rdf:about="http://purl.obolibrary.org/obo/GAZ_00248053">
        <obo:RO_0001025 rdf:resource="http://purl.obolibrary.org/obo/GAZ_00005291"/>
        <obo:IAO_0000115>An island off eastern Abu Dhabi.</obo:IAO_0000115>
        <oboInOwl:hasOBONamespace>GAZ</oboInOwl:hasOBONamespace>
        <oboInOwl:id>GAZ:00248053</oboInOwl:id>
        <rdfs:label>Hayl</rdfs:label>
    </owl:NamedIndividual>
    


    <!-- http://purl.obolibrary.org/obo/GAZ_00248054 -->

    <owl:NamedIndividual rdf:about="http://purl.obolibrary.org/obo/GAZ_00248054">
        <obo:RO_0001025 rdf:resource="http://purl.obolibrary.org/obo/GAZ_00005291"/>
        <obo:IAO_0000115>An island off eastern Abu Dhabi.</obo:IAO_0000115>
        <oboInOwl:hasOBONamespace>GAZ</oboInOwl:hasOBONamespace>
        <oboInOwl:id>GAZ:00248054</oboInOwl:id>
        <rdfs:label>Jazirat Ra&apos;s Ghurab</rdfs:label>
    </owl:NamedIndividual>
    


    <!-- http://purl.obolibrary.org/obo/GAZ_00248055 -->

    <owl:NamedIndividual rdf:about="http://purl.obolibrary.org/obo/GAZ_00248055">
        <obo:RO_0001025 rdf:resource="http://purl.obolibrary.org/obo/GAZ_00005291"/>
        <obo:IAO_0000115>An island off eastern Abu Dhabi.</obo:IAO_0000115>
        <oboInOwl:hasOBONamespace>GAZ</oboInOwl:hasOBONamespace>
        <oboInOwl:id>GAZ:00248055</oboInOwl:id>
        <rdfs:label>Ra&apos;s Ghanadah</rdfs:label>
    </owl:NamedIndividual>
    


    <!-- http://purl.obolibrary.org/obo/GAZ_00248056 -->

    <owl:NamedIndividual rdf:about="http://purl.obolibrary.org/obo/GAZ_00248056">
        <obo:RO_0001025 rdf:resource="http://purl.obolibrary.org/obo/GAZ_00005291"/>
        <obo:IAO_0000115>A group of enriched playa lakes on sabkha, partly maintained by bunding. Located 40 km southeast of Abu Dhabi, in Abu Dhabi Emirate.</obo:IAO_0000115>
        <oboInOwl:hasOBONamespace>GAZ</oboInOwl:hasOBONamespace>
        <oboInOwl:id>GAZ:00248056</oboInOwl:id>
        <rdfs:label>Al Ghar Lakes</rdfs:label>
    </owl:NamedIndividual>
    


    <!-- http://purl.obolibrary.org/obo/GAZ_00248057 -->

    <owl:NamedIndividual rdf:about="http://purl.obolibrary.org/obo/GAZ_00248057">
        <obo:RO_0001025 rdf:resource="http://purl.obolibrary.org/obo/GAZ_00005294"/>
        <obo:IAO_0000115>An island. Located in the Persian Gulf, 75 km from the mainland coast of Abu Dhabi, Abu Dhabi Emirate.</obo:IAO_0000115>
        <oboInOwl:hasOBONamespace>GAZ</oboInOwl:hasOBONamespace>
        <oboInOwl:id>GAZ:00248057</oboInOwl:id>
        <rdfs:label>Sir Bu Nu&apos;ayr</rdfs:label>
    </owl:NamedIndividual>
    


    <!-- http://purl.obolibrary.org/obo/GAZ_00248058 -->

    <owl:NamedIndividual rdf:about="http://purl.obolibrary.org/obo/GAZ_00248058">
        <obo:RO_0001025 rdf:resource="http://purl.obolibrary.org/obo/GAZ_00005289"/>
        <obo:IAO_0000115>A prehistoric extension of Dubai Creek, and consists of saturated salt flats with interspersed sand dunes.</obo:IAO_0000115>
        <oboInOwl:hasOBONamespace>GAZ</oboInOwl:hasOBONamespace>
        <oboInOwl:id>GAZ:00248058</oboInOwl:id>
        <rdfs:label>Zabeel</rdfs:label>
    </owl:NamedIndividual>
    


    <!-- http://purl.obolibrary.org/obo/GAZ_00248059 -->

    <owl:NamedIndividual rdf:about="http://purl.obolibrary.org/obo/GAZ_00248059">
        <obo:RO_0001025 rdf:resource="http://purl.obolibrary.org/obo/GAZ_00005294"/>
        <obo:IAO_0000115>A group of sewage ponds and seepage lagoons with some marsh vegetation, near the coast in Sharjah Emirate. Located 5 km inland, on the border between Sharjah and Ajman Emirates, adjacent to the main coastal highway to Ras al Khaimah, Sharjah Emirate.</obo:IAO_0000115>
        <oboInOwl:hasOBONamespace>GAZ</oboInOwl:hasOBONamespace>
        <oboInOwl:id>GAZ:00248059</oboInOwl:id>
        <rdfs:label>Ramtha Lagoons</rdfs:label>
    </owl:NamedIndividual>
    


    <!-- http://purl.obolibrary.org/obo/GAZ_00248061 -->

    <owl:NamedIndividual rdf:about="http://purl.obolibrary.org/obo/GAZ_00248061">
        <rdf:type rdf:resource="http://purl.obolibrary.org/obo/ENVO_00000475"/>
        <obo:RO_0001025 rdf:resource="http://purl.obolibrary.org/obo/GAZ_00005290"/>
        <obo:IAO_0000115>A tidal creek. An arm of Khor Zawra.</obo:IAO_0000115>
        <oboInOwl:hasOBONamespace>GAZ</oboInOwl:hasOBONamespace>
        <oboInOwl:id>GAZ:00248061</oboInOwl:id>
        <rdfs:label>Khor Zawra</rdfs:label>
    </owl:NamedIndividual>
    


    <!-- http://purl.obolibrary.org/obo/GAZ_00248062 -->

    <owl:NamedIndividual rdf:about="http://purl.obolibrary.org/obo/GAZ_00248062">
        <obo:RO_0001025 rdf:resource="http://purl.obolibrary.org/obo/GAZ_00005292"/>
        <obo:IAO_0000115>A wetland located on the Arabian Gulf coast east of Umm al Qaiwain city and on the landward (southeast) side of Sinaiya Island, Umm al Qaiwain Emirate. It comprises a vast complex of lagoons, 20 km long by an average of 4 km wide, with about 25 low sandy islands, each of less than 50 ha in extent except for the three mangrove-covered round islands of Jazirat al Ghubbah (Ghallah), which are between one and two km in diameter.</obo:IAO_0000115>
        <oboInOwl:hasOBONamespace>GAZ</oboInOwl:hasOBONamespace>
        <oboInOwl:id>GAZ:00248062</oboInOwl:id>
        <rdfs:label>Khor al Beidah</rdfs:label>
    </owl:NamedIndividual>
    


    <!-- http://purl.obolibrary.org/obo/GAZ_00248063 -->

    <owl:NamedIndividual rdf:about="http://purl.obolibrary.org/obo/GAZ_00248063">
        <obo:RO_0001025 rdf:resource="http://purl.obolibrary.org/obo/GAZ_00005292"/>
        <obo:IAO_0000115>An island.</obo:IAO_0000115>
        <oboInOwl:hasOBONamespace>GAZ</oboInOwl:hasOBONamespace>
        <oboInOwl:id>GAZ:00248063</oboInOwl:id>
        <rdfs:label>Jazirat as Siniyah</rdfs:label>
    </owl:NamedIndividual>
    


    <!-- http://purl.obolibrary.org/obo/GAZ_00248064 -->

    <owl:NamedIndividual rdf:about="http://purl.obolibrary.org/obo/GAZ_00248064">
        <obo:RO_0001025 rdf:resource="http://purl.obolibrary.org/obo/GAZ_00005292"/>
        <obo:IAO_0000115>An island.</obo:IAO_0000115>
        <oboInOwl:hasOBONamespace>GAZ</oboInOwl:hasOBONamespace>
        <oboInOwl:id>GAZ:00248064</oboInOwl:id>
        <rdfs:label>Jazirat al Ghallah</rdfs:label>
    </owl:NamedIndividual>
    


    <!-- http://purl.obolibrary.org/obo/GAZ_00248065 -->

    <owl:NamedIndividual rdf:about="http://purl.obolibrary.org/obo/GAZ_00248065">
        <obo:RO_0001025 rdf:resource="http://purl.obolibrary.org/obo/GAZ_00248062"/>
        <obo:IAO_0000115>Three mangrove-covered islands.</obo:IAO_0000115>
        <oboInOwl:hasOBONamespace>GAZ</oboInOwl:hasOBONamespace>
        <oboInOwl:id>GAZ:00248065</oboInOwl:id>
        <rdfs:label>Jazirat al Ghubbah</rdfs:label>
    </owl:NamedIndividual>
    


    <!-- http://purl.obolibrary.org/obo/GAZ_00248066 -->

    <owl:NamedIndividual rdf:about="http://purl.obolibrary.org/obo/GAZ_00248066">
        <obo:RO_0001025 rdf:resource="http://purl.obolibrary.org/obo/GAZ_00248062"/>
        <obo:IAO_0000115>The southwestern portion of the lagoons of Khor al Beidah.</obo:IAO_0000115>
        <oboInOwl:hasOBONamespace>GAZ</oboInOwl:hasOBONamespace>
        <oboInOwl:id>GAZ:00248066</oboInOwl:id>
        <rdfs:label>Khor Umm al Qaiwain</rdfs:label>
    </owl:NamedIndividual>
    


    <!-- http://purl.obolibrary.org/obo/GAZ_00248067 -->

    <owl:NamedIndividual rdf:about="http://purl.obolibrary.org/obo/GAZ_00248067">
        <obo:RO_0001025 rdf:resource="http://purl.obolibrary.org/obo/GAZ_00005293"/>
        <obo:IAO_0000115>A complex of shallow tidal lagoons and inter-tidal mudflats on the Gulf coast, with areas of higher ground covered with halophytic scrub.</obo:IAO_0000115>
        <oboInOwl:hasOBONamespace>GAZ</oboInOwl:hasOBONamespace>
        <oboInOwl:id>GAZ:00248067</oboInOwl:id>
        <rdfs:label>Al Jazeerah Khor</rdfs:label>
    </owl:NamedIndividual>
    


    <!-- http://purl.obolibrary.org/obo/GAZ_00248068 -->

    <owl:NamedIndividual rdf:about="http://purl.obolibrary.org/obo/GAZ_00248068">
        <obo:RO_0001025 rdf:resource="http://purl.obolibrary.org/obo/GAZ_00005293"/>
        <obo:IAO_0000115>An island. Off the W side of the Musandam Peninsula.</obo:IAO_0000115>
        <oboInOwl:hasOBONamespace>GAZ</oboInOwl:hasOBONamespace>
        <oboInOwl:id>GAZ:00248068</oboInOwl:id>
        <rdfs:label>Jazirat Hulaylah</rdfs:label>
    </owl:NamedIndividual>
    


    <!-- http://purl.obolibrary.org/obo/GAZ_00248069 -->

    <owl:NamedIndividual rdf:about="http://purl.obolibrary.org/obo/GAZ_00248069">
        <obo:RO_0001025 rdf:resource="http://purl.obolibrary.org/obo/GAZ_00005293"/>
        <obo:IAO_0000115>An island.</obo:IAO_0000115>
        <oboInOwl:hasOBONamespace>GAZ</oboInOwl:hasOBONamespace>
        <oboInOwl:id>GAZ:00248069</oboInOwl:id>
        <rdfs:label>Jazirat al Hamra&apos;</rdfs:label>
    </owl:NamedIndividual>
    


    <!-- http://purl.obolibrary.org/obo/GAZ_00248070 -->

    <owl:NamedIndividual rdf:about="http://purl.obolibrary.org/obo/GAZ_00248070">
        <obo:RO_0001025 rdf:resource="http://purl.obolibrary.org/obo/GAZ_00005293"/>
        <obo:IAO_0000115>An island.</obo:IAO_0000115>
        <oboInOwl:hasOBONamespace>GAZ</oboInOwl:hasOBONamespace>
        <oboInOwl:id>GAZ:00248070</oboInOwl:id>
        <rdfs:label>Jazirat Qurmah</rdfs:label>
    </owl:NamedIndividual>
    


    <!-- http://purl.obolibrary.org/obo/GAZ_00248071 -->

    <owl:NamedIndividual rdf:about="http://purl.obolibrary.org/obo/GAZ_00248071">
        <obo:IAO_0000115>A bay on the east coast of the UAE in Fujairah and Sharjah Emirates, and straddling the border with Oman.</obo:IAO_0000115>
        <oboInOwl:hasOBONamespace>GAZ</oboInOwl:hasOBONamespace>
        <oboInOwl:id>GAZ:00248071</oboInOwl:id>
        <rdfs:label>Dawhat Diba</rdfs:label>
    </owl:NamedIndividual>
    


    <!-- http://purl.obolibrary.org/obo/GAZ_00248072 -->

    <owl:NamedIndividual rdf:about="http://purl.obolibrary.org/obo/GAZ_00248072">
        <obo:RO_0001025 rdf:resource="http://purl.obolibrary.org/obo/GAZ_00005294"/>
        <obo:IAO_0000115>A man-made dam and reservoir surrounded by steep, desolate mountains which rise to peaks at 900 m. Located in the Hajar Mountains 10 km inland from Khor Fakkan town, Sharjah Emirate.</obo:IAO_0000115>
        <oboInOwl:hasOBONamespace>GAZ</oboInOwl:hasOBONamespace>
        <oboInOwl:id>GAZ:00248072</oboInOwl:id>
        <rdfs:label>Wadi Shih Reservoir</rdfs:label>
    </owl:NamedIndividual>
    


    <!-- http://purl.obolibrary.org/obo/GAZ_00248073 -->

    <owl:NamedIndividual rdf:about="http://purl.obolibrary.org/obo/GAZ_00248073">
        <obo:RO_0001025 rdf:resource="http://purl.obolibrary.org/obo/GAZ_00005288"/>
        <obo:IAO_0000115>A wadi. Located in the Hajar Mountains of Fujairah Emirate. The mouth of the wadi is on the Arabian Sea coast at Qurayyah, 10 km north of Fujairah town and immediately to the north of Fujairah Port.</obo:IAO_0000115>
        <oboInOwl:hasOBONamespace>GAZ</oboInOwl:hasOBONamespace>
        <oboInOwl:id>GAZ:00248073</oboInOwl:id>
        <rdfs:label>Wadi Safad</rdfs:label>
    </owl:NamedIndividual>
    


    <!-- http://purl.obolibrary.org/obo/GAZ_00248074 -->

    <owl:NamedIndividual rdf:about="http://purl.obolibrary.org/obo/GAZ_00248074">
        <obo:RO_0001025 rdf:resource="http://purl.obolibrary.org/obo/GAZ_00005288"/>
        <obo:IAO_0000115>A wadi. Located in the Hajar Mountains of Fujairah Emirate, about 20 km from Fujairah.</obo:IAO_0000115>
        <oboInOwl:hasOBONamespace>GAZ</oboInOwl:hasOBONamespace>
        <oboInOwl:id>GAZ:00248074</oboInOwl:id>
        <rdfs:label>Wadi Hayl</rdfs:label>
    </owl:NamedIndividual>
    


    <!-- http://purl.obolibrary.org/obo/GAZ_00248075 -->

    <owl:NamedIndividual rdf:about="http://purl.obolibrary.org/obo/GAZ_00248075">
        <obo:RO_0001025 rdf:resource="http://purl.obolibrary.org/obo/GAZ_00005294"/>
        <obo:IAO_0000115>A tidal inlet. Khor Kalba is a small, shallow, tidal inlet with ramifying channels formed by the outlet of Wadi Rumh.</obo:IAO_0000115>
        <oboInOwl:hasOBONamespace>GAZ</oboInOwl:hasOBONamespace>
        <oboInOwl:id>GAZ:00248075</oboInOwl:id>
        <rdfs:label>Khor Kalba</rdfs:label>
    </owl:NamedIndividual>
    


    <!-- http://purl.obolibrary.org/obo/GAZ_00248077 -->

    <owl:NamedIndividual rdf:about="http://purl.obolibrary.org/obo/GAZ_00248077">
        <obo:RO_0001025 rdf:resource="http://purl.obolibrary.org/obo/GAZ_00005288"/>
        <obo:IAO_0000115>A wadi. Located on the western flank of the Hajar Mountains in Fujairah Emirate.</obo:IAO_0000115>
        <oboInOwl:hasOBONamespace>GAZ</oboInOwl:hasOBONamespace>
        <oboInOwl:id>GAZ:00248077</oboInOwl:id>
        <rdfs:label>Wadi Ghayl</rdfs:label>
    </owl:NamedIndividual>
    


    <!-- http://purl.obolibrary.org/obo/GAZ_00248078 -->

    <owl:NamedIndividual rdf:about="http://purl.obolibrary.org/obo/GAZ_00248078">
        <obo:RO_0001025 rdf:resource="http://purl.obolibrary.org/obo/GAZ_00005289"/>
        <obo:IAO_0000115>A group of small reservoirs and pools on the western slope of the Flajar Mountains.</obo:IAO_0000115>
        <oboInOwl:hasOBONamespace>GAZ</oboInOwl:hasOBONamespace>
        <oboInOwl:id>GAZ:00248078</oboInOwl:id>
        <rdfs:label>Hatta Lakes</rdfs:label>
    </owl:NamedIndividual>
    


    <!-- http://purl.obolibrary.org/obo/GAZ_00248079 -->

    <owl:NamedIndividual rdf:about="http://purl.obolibrary.org/obo/GAZ_00248079">
        <obo:RO_0001025 rdf:resource="http://purl.obolibrary.org/obo/GAZ_00005291"/>
        <obo:IAO_0000115>A natural spring system much modified by excavation and now with a small permanent lake. Located On the plain to the west of, and immediately adjacent to, Jebel Hafit, and south of Al Am, eastern Abu Dhabi Emirate.</obo:IAO_0000115>
        <oboInOwl:hasOBONamespace>GAZ</oboInOwl:hasOBONamespace>
        <oboInOwl:id>GAZ:00248079</oboInOwl:id>
        <rdfs:label>Ayn al Faydah</rdfs:label>
    </owl:NamedIndividual>
    


    <!-- http://purl.obolibrary.org/obo/GAZ_00248080 -->

    <owl:NamedIndividual rdf:about="http://purl.obolibrary.org/obo/GAZ_00248080">
        <obo:RO_0001025 rdf:resource="http://purl.obolibrary.org/obo/GAZ_00005291"/>
        <obo:IAO_0000115>A group of man-made pools and reed-beds fed by treated sewage and run-off. Part of the Ruwais housing complex of Abu Dhabi National Oil Company (ADNOC), in western Abu Dhabi Emirate.</obo:IAO_0000115>
        <oboInOwl:hasOBONamespace>GAZ</oboInOwl:hasOBONamespace>
        <oboInOwl:id>GAZ:00248080</oboInOwl:id>
        <rdfs:label>Ruwais Reed-beds</rdfs:label>
    </owl:NamedIndividual>
    


    <!-- http://purl.obolibrary.org/obo/GAZ_00250926 -->

    <owl:NamedIndividual rdf:about="http://purl.obolibrary.org/obo/GAZ_00250926">
        <obo:IAO_0000115>A shallow bay.</obo:IAO_0000115>
        <oboInOwl:hasOBONamespace>GAZ</oboInOwl:hasOBONamespace>
        <oboInOwl:id>GAZ:00250926</oboInOwl:id>
        <rdfs:label>Khor Tiab</rdfs:label>
    </owl:NamedIndividual>
    


    <!-- http://purl.obolibrary.org/obo/GAZ_00250927 -->

    <owl:NamedIndividual rdf:about="http://purl.obolibrary.org/obo/GAZ_00250927">
        <obo:IAO_0000115>A shallow bay.</obo:IAO_0000115>
        <oboInOwl:hasOBONamespace>GAZ</oboInOwl:hasOBONamespace>
        <oboInOwl:id>GAZ:00250927</oboInOwl:id>
        <rdfs:label>Khor Kolahy</rdfs:label>
    </owl:NamedIndividual>
    


    <!-- http://purl.obolibrary.org/obo/GAZ_00250973 -->

    <owl:NamedIndividual rdf:about="http://purl.obolibrary.org/obo/GAZ_00250973">
        <obo:IAO_0000115>A large tidal creek. Located north of Jask town in southwest Persian Baluchistan.</obo:IAO_0000115>
        <oboInOwl:hasOBONamespace>GAZ</oboInOwl:hasOBONamespace>
        <oboInOwl:id>GAZ:00250973</oboInOwl:id>
        <rdfs:label>Khowr-e Jask</rdfs:label>
    </owl:NamedIndividual>
    


    <!-- http://purl.obolibrary.org/obo/GAZ_00250974 -->

    <owl:NamedIndividual rdf:about="http://purl.obolibrary.org/obo/GAZ_00250974">
        <obo:IAO_0000115>A river.</obo:IAO_0000115>
        <oboInOwl:hasOBONamespace>GAZ</oboInOwl:hasOBONamespace>
        <oboInOwl:id>GAZ:00250974</oboInOwl:id>
        <rdfs:label>Rud-i-Jagin</rdfs:label>
    </owl:NamedIndividual>
    


    <!-- http://purl.obolibrary.org/obo/GAZ_00250975 -->

    <owl:NamedIndividual rdf:about="http://purl.obolibrary.org/obo/GAZ_00250975">
        <obo:IAO_0000115>A river.</obo:IAO_0000115>
        <oboInOwl:hasOBONamespace>GAZ</oboInOwl:hasOBONamespace>
        <oboInOwl:id>GAZ:00250975</oboInOwl:id>
        <rdfs:label>Rud-i-Gabrik</rdfs:label>
    </owl:NamedIndividual>
    


    <!-- http://purl.obolibrary.org/obo/GAZ_00250979 -->

    <owl:NamedIndividual rdf:about="http://purl.obolibrary.org/obo/GAZ_00250979">
        <obo:IAO_0000115>A river.</obo:IAO_0000115>
        <oboInOwl:hasOBONamespace>GAZ</oboInOwl:hasOBONamespace>
        <oboInOwl:id>GAZ:00250979</oboInOwl:id>
        <rdfs:label>Sarbaz River</rdfs:label>
    </owl:NamedIndividual>
    


    <!-- http://purl.obolibrary.org/obo/GAZ_00250980 -->

    <owl:NamedIndividual rdf:about="http://purl.obolibrary.org/obo/GAZ_00250980">
        <obo:RO_0001025 rdf:resource="http://purl.obolibrary.org/obo/GAZ_00008963"/>
        <obo:IAO_0000115>A bay.</obo:IAO_0000115>
        <oboInOwl:hasOBONamespace>GAZ</oboInOwl:hasOBONamespace>
        <oboInOwl:id>GAZ:00250980</oboInOwl:id>
        <rdfs:label>Khor Govater</rdfs:label>
    </owl:NamedIndividual>
    


    <!-- http://purl.obolibrary.org/obo/GAZ_00415847 -->

    <owl:NamedIndividual rdf:about="http://purl.obolibrary.org/obo/GAZ_00415847">
        <rdf:type rdf:resource="http://purl.obolibrary.org/obo/ENVO_00000856"/>
        <obo:RO_0001025 rdf:resource="http://purl.obolibrary.org/obo/GAZ_00005294"/>
        <obo:IAO_0000115>A populated place. A village that is part of the Emirate of Sharjah in the United Arab Emirates. It is an enclave within the Omani territory of Madha, itself an exclave of Oman.</obo:IAO_0000115>
        <oboInOwl:hasOBONamespace>GAZ</oboInOwl:hasOBONamespace>
        <oboInOwl:id>GAZ:00415847</oboInOwl:id>
        <rdfs:label>Nahwa</rdfs:label>
    </owl:NamedIndividual>
    


    <!-- 
    ///////////////////////////////////////////////////////////////////////////////////////
    //
    // Annotations
    //
    ///////////////////////////////////////////////////////////////////////////////////////
     -->

    <rdf:Description rdf:about="http://purl.obolibrary.org/obo/GAZ_00005287">
        <rdfs:label>Emirate (United Arab Emirates)</rdfs:label>
        <oboInOwl:hasOBONamespace>GAZ</oboInOwl:hasOBONamespace>
        <oboInOwl:id>GAZ:00005287</oboInOwl:id>
    </rdf:Description>
    <rdf:Description rdf:about="http://purl.obolibrary.org/obo/GAZ_00005288">
        <obo:IAO_0000115>One of the seven emirates that make up the United Arab Emirates, on the Gulf of Oman in the country&apos;s east.</obo:IAO_0000115>
        <rdfs:label>Emirate of Fujairah</rdfs:label>
        <oboInOwl:id>GAZ:00005288</oboInOwl:id>
        <oboInOwl:hasOBONamespace>GAZ</oboInOwl:hasOBONamespace>
    </rdf:Description>
    <rdf:Description rdf:about="http://purl.obolibrary.org/obo/GAZ_00005289">
        <rdfs:label>Emirate of Dubai</rdfs:label>
        <obo:IAO_0000115>One of the seven emirates in the United Arab Emirates (UAE). The emirate of Dubai shares borders with Abu Dhabi in the south, Sharjah in the northeast, and the Sultanate of Oman in the southeast. Hatta, a minor exclave of the emirate, is surrounded on three sides by Oman and by the emirates of Ajman (in the west) and Ras Al Khaimah (in the north).</obo:IAO_0000115>
        <oboInOwl:id>GAZ:00005289</oboInOwl:id>
        <oboInOwl:hasOBONamespace>GAZ</oboInOwl:hasOBONamespace>
    </rdf:Description>
    <rdf:Description rdf:about="http://purl.obolibrary.org/obo/GAZ_00005290">
        <obo:IAO_0000115>One of seven emirates comprising the United Arab Emirates (UAE). With an area of just 260 km2, Ajman is the smallest emirate by area. Its seat of government is Ajman, which is bordered to the south by Sharjah and to the north by Umm al-Quwain.</obo:IAO_0000115>
        <oboInOwl:id>GAZ:00005290</oboInOwl:id>
        <oboInOwl:hasOBONamespace>GAZ</oboInOwl:hasOBONamespace>
        <rdfs:label>Emirate of Ajman</rdfs:label>
    </rdf:Description>
    <rdf:Description rdf:about="http://purl.obolibrary.org/obo/GAZ_00005291">
        <rdfs:label>Emirate of Abu Dhabi</rdfs:label>
        <oboInOwl:hasOBONamespace>GAZ</oboInOwl:hasOBONamespace>
        <oboInOwl:id>GAZ:00005291</oboInOwl:id>
        <obo:IAO_0000115>One of seven emirates that constitute the United Arab Emirates (UAE). It adjoins the Kingdom of Saudi Arabia and the Sultanate of Oman. The emirate borders the emirate of Dubai to its north.</obo:IAO_0000115>
    </rdf:Description>
    <rdf:Description rdf:about="http://purl.obolibrary.org/obo/GAZ_00005292">
        <obo:IAO_0000115>One of the emirates in the United Arab Emirates.</obo:IAO_0000115>
        <oboInOwl:hasOBONamespace>GAZ</oboInOwl:hasOBONamespace>
        <rdfs:label>Emirate of Umm al-Quwain</rdfs:label>
        <oboInOwl:id>GAZ:00005292</oboInOwl:id>
    </rdf:Description>
    <rdf:Description rdf:about="http://purl.obolibrary.org/obo/GAZ_00005293">
        <oboInOwl:id>GAZ:00005293</oboInOwl:id>
        <obo:IAO_0000115>One of the emirates of the United Arab Emirates, in the northern part of the Persian gulf.</obo:IAO_0000115>
        <rdfs:label>Emirate of Ras al-Khaimah</rdfs:label>
        <oboInOwl:hasOBONamespace>GAZ</oboInOwl:hasOBONamespace>
    </rdf:Description>
    <rdf:Description rdf:about="http://purl.obolibrary.org/obo/GAZ_00005294">
        <rdfs:label>Emirate of Sharjah</rdfs:label>
        <oboInOwl:hasOBONamespace>GAZ</oboInOwl:hasOBONamespace>
        <oboInOwl:id>GAZ:00005294</oboInOwl:id>
        <obo:IAO_0000115>One of the emirates of the United Arab Emirates (UAE). The emirate of Sharjah comprises the city of Sharjah (the seat of the emirate), and other minor towns and enclaves such as Kalba, Hisn Dibba and Khor Fakkan.</obo:IAO_0000115>
    </rdf:Description>
</rdf:RDF>



<!-- Generated by the OWL API (version 4.5.6) https://github.com/owlcs/owlapi -->

