<?xml version="1.0"?>
<rdf:RDF xmlns="http://purl.obolibrary.org/obo/gaz/subsets/countries/Venezuela.owl#"
     xml:base="http://purl.obolibrary.org/obo/gaz/subsets/countries/Venezuela.owl"
     xmlns:obo="http://purl.obolibrary.org/obo/"
     xmlns:owl="http://www.w3.org/2002/07/owl#"
     xmlns:rdf="http://www.w3.org/1999/02/22-rdf-syntax-ns#"
     xmlns:xml="http://www.w3.org/XML/1998/namespace"
     xmlns:xsd="http://www.w3.org/2001/XMLSchema#"
     xmlns:rdfs="http://www.w3.org/2000/01/rdf-schema#"
     xmlns:oboInOwl="http://www.geneontology.org/formats/oboInOwl#">
    <owl:Ontology rdf:about="http://purl.obolibrary.org/obo/gaz/subsets/countries/Venezuela.owl">
        <owl:imports rdf:resource="http://purl.obolibrary.org/obo/gaz/imports/envo_import.owl"/>
        <owl:imports rdf:resource="http://purl.obolibrary.org/obo/gaz/imports/ro_import.owl"/>
    </owl:Ontology>
    


    <!-- 
    ///////////////////////////////////////////////////////////////////////////////////////
    //
    // Annotation properties
    //
    ///////////////////////////////////////////////////////////////////////////////////////
     -->

    


    <!-- http://purl.obolibrary.org/obo/IAO_0000115 -->

    <owl:AnnotationProperty rdf:about="http://purl.obolibrary.org/obo/IAO_0000115"/>
    


    <!-- http://www.geneontology.org/formats/oboInOwl#hasOBONamespace -->

    <owl:AnnotationProperty rdf:about="http://www.geneontology.org/formats/oboInOwl#hasOBONamespace"/>
    


    <!-- http://www.geneontology.org/formats/oboInOwl#id -->

    <owl:AnnotationProperty rdf:about="http://www.geneontology.org/formats/oboInOwl#id"/>
    


    <!-- 
    ///////////////////////////////////////////////////////////////////////////////////////
    //
    // Object Properties
    //
    ///////////////////////////////////////////////////////////////////////////////////////
     -->

    


    <!-- http://purl.obolibrary.org/obo/RO_0001025 -->

    <owl:ObjectProperty rdf:about="http://purl.obolibrary.org/obo/RO_0001025"/>
    


    <!-- 
    ///////////////////////////////////////////////////////////////////////////////////////
    //
    // Classes
    //
    ///////////////////////////////////////////////////////////////////////////////////////
     -->

    


    <!-- http://purl.obolibrary.org/obo/ENVO_00000009 -->

    <owl:Class rdf:about="http://purl.obolibrary.org/obo/ENVO_00000009"/>
    


    <!-- http://purl.obolibrary.org/obo/ENVO_00000020 -->

    <owl:Class rdf:about="http://purl.obolibrary.org/obo/ENVO_00000020"/>
    


    <!-- http://purl.obolibrary.org/obo/ENVO_00000032 -->

    <owl:Class rdf:about="http://purl.obolibrary.org/obo/ENVO_00000032"/>
    


    <!-- http://purl.obolibrary.org/obo/ENVO_00000098 -->

    <owl:Class rdf:about="http://purl.obolibrary.org/obo/ENVO_00000098"/>
    


    <!-- http://purl.obolibrary.org/obo/ENVO_00000104 -->

    <owl:Class rdf:about="http://purl.obolibrary.org/obo/ENVO_00000104"/>
    


    <!-- http://purl.obolibrary.org/obo/ENVO_00000106 -->

    <owl:Class rdf:about="http://purl.obolibrary.org/obo/ENVO_00000106"/>
    


    <!-- http://purl.obolibrary.org/obo/ENVO_00000191 -->

    <owl:Class rdf:about="http://purl.obolibrary.org/obo/ENVO_00000191"/>
    


    <!-- http://purl.obolibrary.org/obo/ENVO_00000279 -->

    <owl:Class rdf:about="http://purl.obolibrary.org/obo/ENVO_00000279"/>
    


    <!-- http://purl.obolibrary.org/obo/ENVO_00000354 -->

    <owl:Class rdf:about="http://purl.obolibrary.org/obo/ENVO_00000354"/>
    


    <!-- http://purl.obolibrary.org/obo/ENVO_00000398 -->

    <owl:Class rdf:about="http://purl.obolibrary.org/obo/ENVO_00000398"/>
    


    <!-- http://purl.obolibrary.org/obo/ENVO_00000408 -->

    <owl:Class rdf:about="http://purl.obolibrary.org/obo/ENVO_00000408"/>
    


    <!-- http://purl.obolibrary.org/obo/ENVO_00000423 -->

    <owl:Class rdf:about="http://purl.obolibrary.org/obo/ENVO_00000423"/>
    


    <!-- http://purl.obolibrary.org/obo/ENVO_00000856 -->

    <owl:Class rdf:about="http://purl.obolibrary.org/obo/ENVO_00000856"/>
    


    <!-- http://purl.obolibrary.org/obo/GAZ_00009150 -->

    <owl:Class rdf:about="http://purl.obolibrary.org/obo/GAZ_00009150"/>
    


    <!-- http://purl.obolibrary.org/obo/GAZ_00009151 -->

    <owl:Class rdf:about="http://purl.obolibrary.org/obo/GAZ_00009151">
        <rdfs:subClassOf rdf:resource="http://purl.obolibrary.org/obo/GAZ_00009150"/>
    </owl:Class>
    


    <!-- http://purl.obolibrary.org/obo/GAZ_00009152 -->

    <owl:Class rdf:about="http://purl.obolibrary.org/obo/GAZ_00009152"/>
    


    <!-- http://purl.obolibrary.org/obo/GAZ_00011584 -->

    <owl:Class rdf:about="http://purl.obolibrary.org/obo/GAZ_00011584">
        <rdfs:subClassOf rdf:resource="http://purl.obolibrary.org/obo/GAZ_00009150"/>
    </owl:Class>
    


    <!-- http://purl.obolibrary.org/obo/GAZ_00011585 -->

    <owl:Class rdf:about="http://purl.obolibrary.org/obo/GAZ_00011585">
        <rdfs:subClassOf rdf:resource="http://purl.obolibrary.org/obo/GAZ_00009152"/>
    </owl:Class>
    


    <!-- http://purl.obolibrary.org/obo/GAZ_00011587 -->

    <owl:Class rdf:about="http://purl.obolibrary.org/obo/GAZ_00011587">
        <rdfs:subClassOf rdf:resource="http://purl.obolibrary.org/obo/GAZ_00009150"/>
    </owl:Class>
    


    <!-- http://purl.obolibrary.org/obo/GAZ_00011588 -->

    <owl:Class rdf:about="http://purl.obolibrary.org/obo/GAZ_00011588">
        <rdfs:subClassOf rdf:resource="http://purl.obolibrary.org/obo/GAZ_00009150"/>
    </owl:Class>
    


    <!-- http://purl.obolibrary.org/obo/GAZ_00011591 -->

    <owl:Class rdf:about="http://purl.obolibrary.org/obo/GAZ_00011591">
        <rdfs:subClassOf rdf:resource="http://purl.obolibrary.org/obo/GAZ_00009152"/>
    </owl:Class>
    


    <!-- http://purl.obolibrary.org/obo/GAZ_00011592 -->

    <owl:Class rdf:about="http://purl.obolibrary.org/obo/GAZ_00011592">
        <rdfs:subClassOf rdf:resource="http://purl.obolibrary.org/obo/GAZ_00009150"/>
    </owl:Class>
    


    <!-- http://purl.obolibrary.org/obo/GAZ_00011593 -->

    <owl:Class rdf:about="http://purl.obolibrary.org/obo/GAZ_00011593">
        <rdfs:subClassOf rdf:resource="http://purl.obolibrary.org/obo/GAZ_00009152"/>
    </owl:Class>
    


    <!-- http://purl.obolibrary.org/obo/GAZ_00011595 -->

    <owl:Class rdf:about="http://purl.obolibrary.org/obo/GAZ_00011595">
        <rdfs:subClassOf rdf:resource="http://purl.obolibrary.org/obo/GAZ_00009150"/>
    </owl:Class>
    


    <!-- http://purl.obolibrary.org/obo/GAZ_00011598 -->

    <owl:Class rdf:about="http://purl.obolibrary.org/obo/GAZ_00011598">
        <rdfs:subClassOf rdf:resource="http://purl.obolibrary.org/obo/GAZ_00009150"/>
    </owl:Class>
    


    <!-- http://purl.obolibrary.org/obo/GAZ_00011603 -->

    <owl:Class rdf:about="http://purl.obolibrary.org/obo/GAZ_00011603">
        <rdfs:subClassOf rdf:resource="http://purl.obolibrary.org/obo/GAZ_00009152"/>
    </owl:Class>
    


    <!-- http://purl.obolibrary.org/obo/GAZ_00011608 -->

    <owl:Class rdf:about="http://purl.obolibrary.org/obo/GAZ_00011608">
        <rdfs:subClassOf rdf:resource="http://purl.obolibrary.org/obo/GAZ_00009152"/>
    </owl:Class>
    


    <!-- http://purl.obolibrary.org/obo/GAZ_00011612 -->

    <owl:Class rdf:about="http://purl.obolibrary.org/obo/GAZ_00011612">
        <rdfs:subClassOf rdf:resource="http://purl.obolibrary.org/obo/GAZ_00009150"/>
    </owl:Class>
    


    <!-- http://purl.obolibrary.org/obo/GAZ_00011614 -->

    <owl:Class rdf:about="http://purl.obolibrary.org/obo/GAZ_00011614">
        <rdfs:subClassOf rdf:resource="http://purl.obolibrary.org/obo/GAZ_00009150"/>
    </owl:Class>
    


    <!-- http://purl.obolibrary.org/obo/GAZ_00011615 -->

    <owl:Class rdf:about="http://purl.obolibrary.org/obo/GAZ_00011615">
        <rdfs:subClassOf rdf:resource="http://purl.obolibrary.org/obo/GAZ_00009150"/>
    </owl:Class>
    


    <!-- http://purl.obolibrary.org/obo/GAZ_00011616 -->

    <owl:Class rdf:about="http://purl.obolibrary.org/obo/GAZ_00011616">
        <rdfs:subClassOf rdf:resource="http://purl.obolibrary.org/obo/GAZ_00009150"/>
    </owl:Class>
    


    <!-- http://purl.obolibrary.org/obo/GAZ_00011617 -->

    <owl:Class rdf:about="http://purl.obolibrary.org/obo/GAZ_00011617">
        <rdfs:subClassOf rdf:resource="http://purl.obolibrary.org/obo/GAZ_00009150"/>
    </owl:Class>
    


    <!-- http://purl.obolibrary.org/obo/GAZ_00011618 -->

    <owl:Class rdf:about="http://purl.obolibrary.org/obo/GAZ_00011618">
        <rdfs:subClassOf rdf:resource="http://purl.obolibrary.org/obo/GAZ_00009150"/>
    </owl:Class>
    


    <!-- http://purl.obolibrary.org/obo/GAZ_00011620 -->

    <owl:Class rdf:about="http://purl.obolibrary.org/obo/GAZ_00011620">
        <rdfs:subClassOf rdf:resource="http://purl.obolibrary.org/obo/GAZ_00009150"/>
    </owl:Class>
    


    <!-- http://purl.obolibrary.org/obo/GAZ_00011621 -->

    <owl:Class rdf:about="http://purl.obolibrary.org/obo/GAZ_00011621">
        <rdfs:subClassOf rdf:resource="http://purl.obolibrary.org/obo/GAZ_00009150"/>
    </owl:Class>
    


    <!-- http://purl.obolibrary.org/obo/GAZ_00011622 -->

    <owl:Class rdf:about="http://purl.obolibrary.org/obo/GAZ_00011622">
        <rdfs:subClassOf rdf:resource="http://purl.obolibrary.org/obo/GAZ_00009150"/>
    </owl:Class>
    


    <!-- http://purl.obolibrary.org/obo/GAZ_00011623 -->

    <owl:Class rdf:about="http://purl.obolibrary.org/obo/GAZ_00011623">
        <rdfs:subClassOf rdf:resource="http://purl.obolibrary.org/obo/GAZ_00009150"/>
    </owl:Class>
    


    <!-- http://purl.obolibrary.org/obo/GAZ_00011624 -->

    <owl:Class rdf:about="http://purl.obolibrary.org/obo/GAZ_00011624">
        <rdfs:subClassOf rdf:resource="http://purl.obolibrary.org/obo/GAZ_00009150"/>
    </owl:Class>
    


    <!-- http://purl.obolibrary.org/obo/GAZ_00011625 -->

    <owl:Class rdf:about="http://purl.obolibrary.org/obo/GAZ_00011625">
        <rdfs:subClassOf rdf:resource="http://purl.obolibrary.org/obo/GAZ_00009150"/>
    </owl:Class>
    


    <!-- http://purl.obolibrary.org/obo/GAZ_00011626 -->

    <owl:Class rdf:about="http://purl.obolibrary.org/obo/GAZ_00011626">
        <rdfs:subClassOf rdf:resource="http://purl.obolibrary.org/obo/GAZ_00009150"/>
    </owl:Class>
    


    <!-- http://purl.obolibrary.org/obo/GAZ_00011627 -->

    <owl:Class rdf:about="http://purl.obolibrary.org/obo/GAZ_00011627">
        <rdfs:subClassOf rdf:resource="http://purl.obolibrary.org/obo/GAZ_00009150"/>
    </owl:Class>
    


    <!-- http://purl.obolibrary.org/obo/GAZ_00011628 -->

    <owl:Class rdf:about="http://purl.obolibrary.org/obo/GAZ_00011628">
        <rdfs:subClassOf rdf:resource="http://purl.obolibrary.org/obo/GAZ_00009150"/>
    </owl:Class>
    


    <!-- http://purl.obolibrary.org/obo/GAZ_00011629 -->

    <owl:Class rdf:about="http://purl.obolibrary.org/obo/GAZ_00011629">
        <rdfs:subClassOf rdf:resource="http://purl.obolibrary.org/obo/GAZ_00009150"/>
    </owl:Class>
    


    <!-- http://purl.obolibrary.org/obo/GAZ_02000849 -->

    <owl:Class rdf:about="http://purl.obolibrary.org/obo/GAZ_02000849">
        <rdfs:subClassOf rdf:resource="http://purl.obolibrary.org/obo/GAZ_00009152"/>
    </owl:Class>
    


    <!-- 
    ///////////////////////////////////////////////////////////////////////////////////////
    //
    // Individuals
    //
    ///////////////////////////////////////////////////////////////////////////////////////
     -->

    


    <!-- http://purl.obolibrary.org/obo/GAZ_00002931 -->

    <owl:NamedIndividual rdf:about="http://purl.obolibrary.org/obo/GAZ_00002931">
        <rdf:type rdf:resource="http://purl.obolibrary.org/obo/ENVO_00000009"/>
        <obo:IAO_0000115>A country on the northern coast of South America. The country comprises a continental mainland and numerous islands located off the Venezuelan coastline in the Caribbean Sea. The Bolivarian Republic of Venezuela possesses borders with Guyana to the east, Brazil to the south, and Colombia to the west. Trinidad and Tobago, Grenada, St. Lucia, Barbados, Curacao, Bonaire, Aruba, Saint Vincent and the Grenadines and the Leeward Antilles lie just north, off the Venezuelan coast. Venezuela is divided into twenty-three states (Estados), a capital district (distrito capital) corresponding to the city of Caracas, the Federal Dependencies (Dependencias Federales, a special territory), and Guayana Esequiba (claimed in a border dispute with Guyana). Venezuela is further subdivided into 335 municipalities (municipios); these are subdivided into over one thousand parishes (parroquias).</obo:IAO_0000115>
        <oboInOwl:hasOBONamespace>GAZ</oboInOwl:hasOBONamespace>
        <oboInOwl:id>GAZ:00002931</oboInOwl:id>
        <rdfs:label>Venezuela</rdfs:label>
    </owl:NamedIndividual>
    


    <!-- http://purl.obolibrary.org/obo/GAZ_00004639 -->

    <owl:NamedIndividual rdf:about="http://purl.obolibrary.org/obo/GAZ_00004639">
        <obo:IAO_0000115>A national park located in the Andes, in Llanquihue Province, in Los Lagos Region of Chile. The park is adjacent to Puyehue National Park and Nahuel Huapi National Park (Argentina). In addition to, Petrohue River separates it from Llanquihue National Reserve.</obo:IAO_0000115>
        <oboInOwl:hasOBONamespace>GAZ</oboInOwl:hasOBONamespace>
        <oboInOwl:id>GAZ:00004639</oboInOwl:id>
        <rdfs:label>Parque Nacional Vicente Perez Rosales</rdfs:label>
    </owl:NamedIndividual>
    


    <!-- http://purl.obolibrary.org/obo/GAZ_00004640 -->

    <owl:NamedIndividual rdf:about="http://purl.obolibrary.org/obo/GAZ_00004640">
        <obo:RO_0001025 rdf:resource="http://purl.obolibrary.org/obo/GAZ_00004639"/>
        <obo:RO_0001025 rdf:resource="http://purl.obolibrary.org/obo/GAZ_00136453"/>
        <obo:IAO_0000115>An eroded stratovolcano.</obo:IAO_0000115>
        <oboInOwl:hasOBONamespace>GAZ</oboInOwl:hasOBONamespace>
        <oboInOwl:id>GAZ:00004640</oboInOwl:id>
        <rdfs:label>La Picada</rdfs:label>
    </owl:NamedIndividual>
    


    <!-- http://purl.obolibrary.org/obo/GAZ_00005073 -->

    <owl:NamedIndividual rdf:about="http://purl.obolibrary.org/obo/GAZ_00005073">
        <rdf:type rdf:resource="http://purl.obolibrary.org/obo/ENVO_00000856"/>
        <obo:RO_0001025 rdf:resource="http://purl.obolibrary.org/obo/GAZ_00009151"/>
        <obo:IAO_0000115>A municipality located in Anzoategui State, Venezuela, in the northeastern part of the country and on the Caribbean coast.</obo:IAO_0000115>
        <oboInOwl:hasOBONamespace>GAZ</oboInOwl:hasOBONamespace>
        <oboInOwl:id>GAZ:00005073</oboInOwl:id>
        <rdfs:label>Municipality of Guanta</rdfs:label>
    </owl:NamedIndividual>
    


    <!-- http://purl.obolibrary.org/obo/GAZ_00007836 -->

    <owl:NamedIndividual rdf:about="http://purl.obolibrary.org/obo/GAZ_00007836">
        <obo:RO_0001025 rdf:resource="http://purl.obolibrary.org/obo/GAZ_00056736"/>
        <obo:IAO_0000115>A large brackish bay in Venezuela at 10deg39minN, 71deg36minW. It is connected to the Gulf of Venezuela by a 55 km strait on the northern edge of the lake, and fed by numerous rivers, the largest being the Catatumbo River.</obo:IAO_0000115>
        <oboInOwl:hasOBONamespace>GAZ</oboInOwl:hasOBONamespace>
        <oboInOwl:id>GAZ:00007836</oboInOwl:id>
        <rdfs:label>Lake Maracaibo</rdfs:label>
    </owl:NamedIndividual>
    


    <!-- http://purl.obolibrary.org/obo/GAZ_00008039 -->

    <owl:NamedIndividual rdf:about="http://purl.obolibrary.org/obo/GAZ_00008039">
        <obo:RO_0001025 rdf:resource="http://purl.obolibrary.org/obo/GAZ_00002931"/>
        <obo:IAO_0000115>A river in S. America. The Orinoco course describes a wide ellipsoidal arc, surrounding the Guiana Shield; it is divided in four stretches of unequal length that roughly correspond to the longitudinal zonation of a typical large river.</obo:IAO_0000115>
        <oboInOwl:hasOBONamespace>GAZ</oboInOwl:hasOBONamespace>
        <oboInOwl:id>GAZ:00008039</oboInOwl:id>
        <rdfs:label>Orinoco River</rdfs:label>
    </owl:NamedIndividual>
    


    <!-- http://purl.obolibrary.org/obo/GAZ_00008749 -->

    <owl:NamedIndividual rdf:about="http://purl.obolibrary.org/obo/GAZ_00008749">
        <obo:RO_0001025 rdf:resource="http://purl.obolibrary.org/obo/GAZ_00136449"/>
        <obo:IAO_0000115>A geyser field located within the Andes Mountains of northern Chile at 4,200 meters above mean sea level. A chain of dominantly Pliocene-to-Pleistocene volcanoes including Cerro Deslinde, Cerro Volcan, Cerros del Tatio, and Volcan Tatio is flanked on the west by a depression that contains some of the most dramatic thermal features of the Andes. The 30 km2 Hoyada de Los Geisers del Tatio geothermal field contains 85 fumaroles and solfataras, 62 hot springs, 40 geysers, 5 mud volcanoes, and extensive sinter terraces.</obo:IAO_0000115>
        <oboInOwl:hasOBONamespace>GAZ</oboInOwl:hasOBONamespace>
        <oboInOwl:id>GAZ:00008749</oboInOwl:id>
        <rdfs:label>El Tatio Geyser Field</rdfs:label>
    </owl:NamedIndividual>
    


    <!-- http://purl.obolibrary.org/obo/GAZ_00009150 -->

    <owl:NamedIndividual rdf:about="http://purl.obolibrary.org/obo/GAZ_00009150">
        <obo:RO_0001025 rdf:resource="http://purl.obolibrary.org/obo/GAZ_00002931"/>
    </owl:NamedIndividual>
    


    <!-- http://purl.obolibrary.org/obo/GAZ_00009151 -->

    <owl:NamedIndividual rdf:about="http://purl.obolibrary.org/obo/GAZ_00009151"/>
    


    <!-- http://purl.obolibrary.org/obo/GAZ_00009152 -->

    <owl:NamedIndividual rdf:about="http://purl.obolibrary.org/obo/GAZ_00009152">
        <obo:RO_0001025 rdf:resource="http://purl.obolibrary.org/obo/GAZ_00002931"/>
    </owl:NamedIndividual>
    


    <!-- http://purl.obolibrary.org/obo/GAZ_00011584 -->

    <owl:NamedIndividual rdf:about="http://purl.obolibrary.org/obo/GAZ_00011584"/>
    


    <!-- http://purl.obolibrary.org/obo/GAZ_00011585 -->

    <owl:NamedIndividual rdf:about="http://purl.obolibrary.org/obo/GAZ_00011585">
        <obo:RO_0001025 rdf:resource="http://purl.obolibrary.org/obo/GAZ_04000006"/>
    </owl:NamedIndividual>
    


    <!-- http://purl.obolibrary.org/obo/GAZ_00011586 -->

    <owl:NamedIndividual rdf:about="http://purl.obolibrary.org/obo/GAZ_00011586">
        <obo:RO_0001025 rdf:resource="http://purl.obolibrary.org/obo/GAZ_04000007"/>
        <oboInOwl:hasOBONamespace>GAZ</oboInOwl:hasOBONamespace>
        <oboInOwl:id>GAZ:00011586</oboInOwl:id>
        <rdfs:label>Recreo</rdfs:label>
    </owl:NamedIndividual>
    


    <!-- http://purl.obolibrary.org/obo/GAZ_00011587 -->

    <owl:NamedIndividual rdf:about="http://purl.obolibrary.org/obo/GAZ_00011587"/>
    


    <!-- http://purl.obolibrary.org/obo/GAZ_00011588 -->

    <owl:NamedIndividual rdf:about="http://purl.obolibrary.org/obo/GAZ_00011588"/>
    


    <!-- http://purl.obolibrary.org/obo/GAZ_00011589 -->

    <owl:NamedIndividual rdf:about="http://purl.obolibrary.org/obo/GAZ_00011589">
        <obo:RO_0001025 rdf:resource="http://purl.obolibrary.org/obo/GAZ_04000008"/>
        <obo:IAO_0000115>A populated place.</obo:IAO_0000115>
        <oboInOwl:hasOBONamespace>GAZ</oboInOwl:hasOBONamespace>
        <oboInOwl:id>GAZ:00011589</oboInOwl:id>
        <rdfs:label>Arismendi</rdfs:label>
    </owl:NamedIndividual>
    


    <!-- http://purl.obolibrary.org/obo/GAZ_00011590 -->

    <owl:NamedIndividual rdf:about="http://purl.obolibrary.org/obo/GAZ_00011590">
        <obo:RO_0001025 rdf:resource="http://purl.obolibrary.org/obo/GAZ_00002931"/>
        <oboInOwl:hasOBONamespace>GAZ</oboInOwl:hasOBONamespace>
        <oboInOwl:id>GAZ:00011590</oboInOwl:id>
        <rdfs:label>Capital District (Venezuala)</rdfs:label>
    </owl:NamedIndividual>
    


    <!-- http://purl.obolibrary.org/obo/GAZ_00011591 -->

    <owl:NamedIndividual rdf:about="http://purl.obolibrary.org/obo/GAZ_00011591">
        <obo:RO_0001025 rdf:resource="http://purl.obolibrary.org/obo/GAZ_00011590"/>
    </owl:NamedIndividual>
    


    <!-- http://purl.obolibrary.org/obo/GAZ_00011592 -->

    <owl:NamedIndividual rdf:about="http://purl.obolibrary.org/obo/GAZ_00011592"/>
    


    <!-- http://purl.obolibrary.org/obo/GAZ_00011593 -->

    <owl:NamedIndividual rdf:about="http://purl.obolibrary.org/obo/GAZ_00011593">
        <obo:RO_0001025 rdf:resource="http://purl.obolibrary.org/obo/GAZ_04000009"/>
    </owl:NamedIndividual>
    


    <!-- http://purl.obolibrary.org/obo/GAZ_00011594 -->

    <owl:NamedIndividual rdf:about="http://purl.obolibrary.org/obo/GAZ_00011594">
        <obo:RO_0001025 rdf:resource="http://purl.obolibrary.org/obo/GAZ_00011592"/>
        <oboInOwl:hasOBONamespace>GAZ</oboInOwl:hasOBONamespace>
        <oboInOwl:id>GAZ:00011594</oboInOwl:id>
        <rdfs:label>Hondo</rdfs:label>
    </owl:NamedIndividual>
    


    <!-- http://purl.obolibrary.org/obo/GAZ_00011595 -->

    <owl:NamedIndividual rdf:about="http://purl.obolibrary.org/obo/GAZ_00011595"/>
    


    <!-- http://purl.obolibrary.org/obo/GAZ_00011596 -->

    <owl:NamedIndividual rdf:about="http://purl.obolibrary.org/obo/GAZ_00011596">
        <obo:RO_0001025 rdf:resource="http://purl.obolibrary.org/obo/GAZ_00011595"/>
        <oboInOwl:hasOBONamespace>GAZ</oboInOwl:hasOBONamespace>
        <oboInOwl:id>GAZ:00011596</oboInOwl:id>
        <rdfs:label>Palo Seco</rdfs:label>
    </owl:NamedIndividual>
    


    <!-- http://purl.obolibrary.org/obo/GAZ_00011597 -->

    <owl:NamedIndividual rdf:about="http://purl.obolibrary.org/obo/GAZ_00011597">
        <obo:RO_0001025 rdf:resource="http://purl.obolibrary.org/obo/GAZ_22223489"/>
        <oboInOwl:hasOBONamespace>GAZ</oboInOwl:hasOBONamespace>
        <oboInOwl:id>GAZ:00011597</oboInOwl:id>
        <rdfs:label>Mara</rdfs:label>
    </owl:NamedIndividual>
    


    <!-- http://purl.obolibrary.org/obo/GAZ_00011598 -->

    <owl:NamedIndividual rdf:about="http://purl.obolibrary.org/obo/GAZ_00011598"/>
    


    <!-- http://purl.obolibrary.org/obo/GAZ_00011599 -->

    <owl:NamedIndividual rdf:about="http://purl.obolibrary.org/obo/GAZ_00011599">
        <obo:RO_0001025 rdf:resource="http://purl.obolibrary.org/obo/GAZ_00011598"/>
        <oboInOwl:hasOBONamespace>GAZ</oboInOwl:hasOBONamespace>
        <oboInOwl:id>GAZ:00011599</oboInOwl:id>
        <rdfs:label>Municipality of Guanarito</rdfs:label>
    </owl:NamedIndividual>
    


    <!-- http://purl.obolibrary.org/obo/GAZ_00011600 -->

    <owl:NamedIndividual rdf:about="http://purl.obolibrary.org/obo/GAZ_00011600">
        <obo:RO_0001025 rdf:resource="http://purl.obolibrary.org/obo/GAZ_00011599"/>
        <oboInOwl:hasOBONamespace>GAZ</oboInOwl:hasOBONamespace>
        <oboInOwl:id>GAZ:00011600</oboInOwl:id>
        <rdfs:label>La Trinidad de la Capilla</rdfs:label>
    </owl:NamedIndividual>
    


    <!-- http://purl.obolibrary.org/obo/GAZ_00011601 -->

    <owl:NamedIndividual rdf:about="http://purl.obolibrary.org/obo/GAZ_00011601">
        <obo:RO_0001025 rdf:resource="http://purl.obolibrary.org/obo/GAZ_00011598"/>
        <oboInOwl:hasOBONamespace>GAZ</oboInOwl:hasOBONamespace>
        <oboInOwl:id>GAZ:00011601</oboInOwl:id>
        <rdfs:label>El Chorrosco</rdfs:label>
    </owl:NamedIndividual>
    


    <!-- http://purl.obolibrary.org/obo/GAZ_00011602 -->

    <owl:NamedIndividual rdf:about="http://purl.obolibrary.org/obo/GAZ_00011602">
        <obo:RO_0001025 rdf:resource="http://purl.obolibrary.org/obo/GAZ_00011598"/>
        <oboInOwl:hasOBONamespace>GAZ</oboInOwl:hasOBONamespace>
        <oboInOwl:id>GAZ:00011602</oboInOwl:id>
        <rdfs:label>Banco de Marones</rdfs:label>
    </owl:NamedIndividual>
    


    <!-- http://purl.obolibrary.org/obo/GAZ_00011603 -->

    <owl:NamedIndividual rdf:about="http://purl.obolibrary.org/obo/GAZ_00011603">
        <obo:RO_0001025 rdf:resource="http://purl.obolibrary.org/obo/GAZ_04000010"/>
    </owl:NamedIndividual>
    


    <!-- http://purl.obolibrary.org/obo/GAZ_00011604 -->

    <owl:NamedIndividual rdf:about="http://purl.obolibrary.org/obo/GAZ_00011604">
        <obo:RO_0001025 rdf:resource="http://purl.obolibrary.org/obo/GAZ_00011598"/>
        <oboInOwl:hasOBONamespace>GAZ</oboInOwl:hasOBONamespace>
        <oboInOwl:id>GAZ:00011604</oboInOwl:id>
        <rdfs:label>La Capilla</rdfs:label>
    </owl:NamedIndividual>
    


    <!-- http://purl.obolibrary.org/obo/GAZ_00011605 -->

    <owl:NamedIndividual rdf:about="http://purl.obolibrary.org/obo/GAZ_00011605">
        <obo:RO_0001025 rdf:resource="http://purl.obolibrary.org/obo/GAZ_00011598"/>
        <obo:IAO_0000115>A populated place.</obo:IAO_0000115>
        <oboInOwl:hasOBONamespace>GAZ</oboInOwl:hasOBONamespace>
        <oboInOwl:id>GAZ:00011605</oboInOwl:id>
        <rdfs:label>La Espinalua</rdfs:label>
    </owl:NamedIndividual>
    


    <!-- http://purl.obolibrary.org/obo/GAZ_00011606 -->

    <owl:NamedIndividual rdf:about="http://purl.obolibrary.org/obo/GAZ_00011606">
        <obo:RO_0001025 rdf:resource="http://purl.obolibrary.org/obo/GAZ_00011598"/>
        <obo:IAO_0000115>A populated place.</obo:IAO_0000115>
        <oboInOwl:hasOBONamespace>GAZ</oboInOwl:hasOBONamespace>
        <oboInOwl:id>GAZ:00011606</oboInOwl:id>
        <rdfs:label>Cano Delgadito</rdfs:label>
    </owl:NamedIndividual>
    


    <!-- http://purl.obolibrary.org/obo/GAZ_00011607 -->

    <owl:NamedIndividual rdf:about="http://purl.obolibrary.org/obo/GAZ_00011607">
        <obo:RO_0001025 rdf:resource="http://purl.obolibrary.org/obo/GAZ_00011598"/>
        <oboInOwl:hasOBONamespace>GAZ</oboInOwl:hasOBONamespace>
        <oboInOwl:id>GAZ:00011607</oboInOwl:id>
        <rdfs:label>Map</rdfs:label>
    </owl:NamedIndividual>
    


    <!-- http://purl.obolibrary.org/obo/GAZ_00011608 -->

    <owl:NamedIndividual rdf:about="http://purl.obolibrary.org/obo/GAZ_00011608">
        <obo:RO_0001025 rdf:resource="http://purl.obolibrary.org/obo/GAZ_00011598"/>
        <obo:RO_0001025 rdf:resource="http://purl.obolibrary.org/obo/GAZ_04000007"/>
    </owl:NamedIndividual>
    


    <!-- http://purl.obolibrary.org/obo/GAZ_00011609 -->

    <owl:NamedIndividual rdf:about="http://purl.obolibrary.org/obo/GAZ_00011609">
        <obo:RO_0001025 rdf:resource="http://purl.obolibrary.org/obo/GAZ_04000011"/>
        <oboInOwl:hasOBONamespace>GAZ</oboInOwl:hasOBONamespace>
        <oboInOwl:id>GAZ:00011609</oboInOwl:id>
        <rdfs:label>Pirital</rdfs:label>
    </owl:NamedIndividual>
    


    <!-- http://purl.obolibrary.org/obo/GAZ_00011610 -->

    <owl:NamedIndividual rdf:about="http://purl.obolibrary.org/obo/GAZ_00011610">
        <obo:RO_0001025 rdf:resource="http://purl.obolibrary.org/obo/GAZ_00011598"/>
        <oboInOwl:hasOBONamespace>GAZ</oboInOwl:hasOBONamespace>
        <oboInOwl:id>GAZ:00011610</oboInOwl:id>
        <rdfs:label>Maporita</rdfs:label>
    </owl:NamedIndividual>
    


    <!-- http://purl.obolibrary.org/obo/GAZ_00011611 -->

    <owl:NamedIndividual rdf:about="http://purl.obolibrary.org/obo/GAZ_00011611">
        <obo:RO_0001025 rdf:resource="http://purl.obolibrary.org/obo/GAZ_00011598"/>
        <oboInOwl:hasOBONamespace>GAZ</oboInOwl:hasOBONamespace>
        <oboInOwl:id>GAZ:00011611</oboInOwl:id>
        <rdfs:label>Quebrada la Virgin</rdfs:label>
    </owl:NamedIndividual>
    


    <!-- http://purl.obolibrary.org/obo/GAZ_00011612 -->

    <owl:NamedIndividual rdf:about="http://purl.obolibrary.org/obo/GAZ_00011612"/>
    


    <!-- http://purl.obolibrary.org/obo/GAZ_00011614 -->

    <owl:NamedIndividual rdf:about="http://purl.obolibrary.org/obo/GAZ_00011614"/>
    


    <!-- http://purl.obolibrary.org/obo/GAZ_00011615 -->

    <owl:NamedIndividual rdf:about="http://purl.obolibrary.org/obo/GAZ_00011615"/>
    


    <!-- http://purl.obolibrary.org/obo/GAZ_00011616 -->

    <owl:NamedIndividual rdf:about="http://purl.obolibrary.org/obo/GAZ_00011616"/>
    


    <!-- http://purl.obolibrary.org/obo/GAZ_00011617 -->

    <owl:NamedIndividual rdf:about="http://purl.obolibrary.org/obo/GAZ_00011617"/>
    


    <!-- http://purl.obolibrary.org/obo/GAZ_00011618 -->

    <owl:NamedIndividual rdf:about="http://purl.obolibrary.org/obo/GAZ_00011618"/>
    


    <!-- http://purl.obolibrary.org/obo/GAZ_00011619 -->

    <owl:NamedIndividual rdf:about="http://purl.obolibrary.org/obo/GAZ_00011619">
        <obo:RO_0001025 rdf:resource="http://purl.obolibrary.org/obo/GAZ_00002931"/>
        <oboInOwl:hasOBONamespace>GAZ</oboInOwl:hasOBONamespace>
        <oboInOwl:id>GAZ:00011619</oboInOwl:id>
        <rdfs:label>Federal Dependency (Venezuala)</rdfs:label>
    </owl:NamedIndividual>
    


    <!-- http://purl.obolibrary.org/obo/GAZ_00011620 -->

    <owl:NamedIndividual rdf:about="http://purl.obolibrary.org/obo/GAZ_00011620"/>
    


    <!-- http://purl.obolibrary.org/obo/GAZ_00011621 -->

    <owl:NamedIndividual rdf:about="http://purl.obolibrary.org/obo/GAZ_00011621"/>
    


    <!-- http://purl.obolibrary.org/obo/GAZ_00011622 -->

    <owl:NamedIndividual rdf:about="http://purl.obolibrary.org/obo/GAZ_00011622"/>
    


    <!-- http://purl.obolibrary.org/obo/GAZ_00011623 -->

    <owl:NamedIndividual rdf:about="http://purl.obolibrary.org/obo/GAZ_00011623"/>
    


    <!-- http://purl.obolibrary.org/obo/GAZ_00011624 -->

    <owl:NamedIndividual rdf:about="http://purl.obolibrary.org/obo/GAZ_00011624"/>
    


    <!-- http://purl.obolibrary.org/obo/GAZ_00011625 -->

    <owl:NamedIndividual rdf:about="http://purl.obolibrary.org/obo/GAZ_00011625"/>
    


    <!-- http://purl.obolibrary.org/obo/GAZ_00011626 -->

    <owl:NamedIndividual rdf:about="http://purl.obolibrary.org/obo/GAZ_00011626"/>
    


    <!-- http://purl.obolibrary.org/obo/GAZ_00011627 -->

    <owl:NamedIndividual rdf:about="http://purl.obolibrary.org/obo/GAZ_00011627"/>
    


    <!-- http://purl.obolibrary.org/obo/GAZ_00011628 -->

    <owl:NamedIndividual rdf:about="http://purl.obolibrary.org/obo/GAZ_00011628"/>
    


    <!-- http://purl.obolibrary.org/obo/GAZ_00011629 -->

    <owl:NamedIndividual rdf:about="http://purl.obolibrary.org/obo/GAZ_00011629"/>
    


    <!-- http://purl.obolibrary.org/obo/GAZ_00011630 -->

    <owl:NamedIndividual rdf:about="http://purl.obolibrary.org/obo/GAZ_00011630">
        <obo:RO_0001025 rdf:resource="http://purl.obolibrary.org/obo/GAZ_00011619"/>
        <oboInOwl:hasOBONamespace>GAZ</oboInOwl:hasOBONamespace>
        <oboInOwl:id>GAZ:00011630</oboInOwl:id>
        <rdfs:label>Isla La Sola</rdfs:label>
    </owl:NamedIndividual>
    


    <!-- http://purl.obolibrary.org/obo/GAZ_00011631 -->

    <owl:NamedIndividual rdf:about="http://purl.obolibrary.org/obo/GAZ_00011631">
        <obo:RO_0001025 rdf:resource="http://purl.obolibrary.org/obo/GAZ_00011619"/>
        <obo:IAO_0000115>A chain of seven rocky barren islets that is part of the Federal Dependencies of Venezuela.</obo:IAO_0000115>
        <oboInOwl:hasOBONamespace>GAZ</oboInOwl:hasOBONamespace>
        <oboInOwl:id>GAZ:00011631</oboInOwl:id>
        <rdfs:label>Los Hermanos Archipelago</rdfs:label>
    </owl:NamedIndividual>
    


    <!-- http://purl.obolibrary.org/obo/GAZ_00011632 -->

    <owl:NamedIndividual rdf:about="http://purl.obolibrary.org/obo/GAZ_00011632">
        <rdf:type rdf:resource="http://purl.obolibrary.org/obo/ENVO_00000098"/>
        <obo:RO_0001025 rdf:resource="http://purl.obolibrary.org/obo/GAZ_00011619"/>
        <obo:IAO_0000115>A Caribbean islet whose status is the subject of a territorial dispute between Dominica and Venezuela. It lies to the west of the Leeward Islands chain. It is sometimes completely submerged during hurricanes. It is 115 miles southwest of Montserrat, 70 miles west of Dominica and 340 miles north of the Venezuelan mainland.</obo:IAO_0000115>
        <oboInOwl:hasOBONamespace>GAZ</oboInOwl:hasOBONamespace>
        <oboInOwl:id>GAZ:00011632</oboInOwl:id>
        <rdfs:label>Isla de Aves</rdfs:label>
    </owl:NamedIndividual>
    


    <!-- http://purl.obolibrary.org/obo/GAZ_00011633 -->

    <owl:NamedIndividual rdf:about="http://purl.obolibrary.org/obo/GAZ_00011633">
        <obo:RO_0001025 rdf:resource="http://purl.obolibrary.org/obo/GAZ_00011619"/>
        <obo:IAO_0000115>An archipelago located to the north west of the Gulf of Venezuela off the coast of Colombia.</obo:IAO_0000115>
        <oboInOwl:hasOBONamespace>GAZ</oboInOwl:hasOBONamespace>
        <oboInOwl:id>GAZ:00011633</oboInOwl:id>
        <rdfs:label>Los Monjes Archipelago</rdfs:label>
    </owl:NamedIndividual>
    


    <!-- http://purl.obolibrary.org/obo/GAZ_00011634 -->

    <owl:NamedIndividual rdf:about="http://purl.obolibrary.org/obo/GAZ_00011634">
        <obo:RO_0001025 rdf:resource="http://purl.obolibrary.org/obo/GAZ_00011619"/>
        <obo:IAO_0000115>An archipelago located north of the Venezuelan states of Aragua and Carabobo, between Bonaire in the west, and the Los Roques Archipelago in the east. The archipelago consists of two atoll-like reef complexes.</obo:IAO_0000115>
        <oboInOwl:hasOBONamespace>GAZ</oboInOwl:hasOBONamespace>
        <oboInOwl:id>GAZ:00011634</oboInOwl:id>
        <rdfs:label>Las Aves Archipelago</rdfs:label>
    </owl:NamedIndividual>
    


    <!-- http://purl.obolibrary.org/obo/GAZ_00011635 -->

    <owl:NamedIndividual rdf:about="http://purl.obolibrary.org/obo/GAZ_00011635">
        <obo:RO_0001025 rdf:resource="http://purl.obolibrary.org/obo/GAZ_00011619"/>
        <obo:IAO_0000115>An archipelago of rock islets with sparse scrub vegetation belonging to the Federal dependencies of Venezuela, part of Venezuela.</obo:IAO_0000115>
        <oboInOwl:hasOBONamespace>GAZ</oboInOwl:hasOBONamespace>
        <oboInOwl:id>GAZ:00011635</oboInOwl:id>
        <rdfs:label>Los Frailes Archipelago</rdfs:label>
    </owl:NamedIndividual>
    


    <!-- http://purl.obolibrary.org/obo/GAZ_00011636 -->

    <owl:NamedIndividual rdf:about="http://purl.obolibrary.org/obo/GAZ_00011636">
        <obo:RO_0001025 rdf:resource="http://purl.obolibrary.org/obo/GAZ_00011619"/>
        <obo:IAO_0000115>An island, one of the federal dependencies of Venezuela, located in the southeastern Caribbean Sea about 182 miles northeast of Caracas.</obo:IAO_0000115>
        <oboInOwl:hasOBONamespace>GAZ</oboInOwl:hasOBONamespace>
        <oboInOwl:id>GAZ:00011636</oboInOwl:id>
        <rdfs:label>Blanquilla Island</rdfs:label>
    </owl:NamedIndividual>
    


    <!-- http://purl.obolibrary.org/obo/GAZ_00011637 -->

    <owl:NamedIndividual rdf:about="http://purl.obolibrary.org/obo/GAZ_00011637">
        <obo:RO_0001025 rdf:resource="http://purl.obolibrary.org/obo/GAZ_00011619"/>
        <oboInOwl:hasOBONamespace>GAZ</oboInOwl:hasOBONamespace>
        <oboInOwl:id>GAZ:00011637</oboInOwl:id>
        <rdfs:label>Isla de Patos</rdfs:label>
    </owl:NamedIndividual>
    


    <!-- http://purl.obolibrary.org/obo/GAZ_00011638 -->

    <owl:NamedIndividual rdf:about="http://purl.obolibrary.org/obo/GAZ_00011638">
        <obo:RO_0001025 rdf:resource="http://purl.obolibrary.org/obo/GAZ_00011619"/>
        <obo:IAO_0000115>An archipelago consisting of about 50 islands, cays or islets. The archipelago is an atoll located some 145 km directly north of the port of La Guaira, close to Caracas.</obo:IAO_0000115>
        <oboInOwl:hasOBONamespace>GAZ</oboInOwl:hasOBONamespace>
        <oboInOwl:id>GAZ:00011638</oboInOwl:id>
        <rdfs:label>Los Roques Archipelago</rdfs:label>
    </owl:NamedIndividual>
    


    <!-- http://purl.obolibrary.org/obo/GAZ_00011640 -->

    <owl:NamedIndividual rdf:about="http://purl.obolibrary.org/obo/GAZ_00011640">
        <obo:RO_0001025 rdf:resource="http://purl.obolibrary.org/obo/GAZ_00011619"/>
        <oboInOwl:hasOBONamespace>GAZ</oboInOwl:hasOBONamespace>
        <oboInOwl:id>GAZ:00011640</oboInOwl:id>
        <rdfs:label>Los Testigos Islands</rdfs:label>
    </owl:NamedIndividual>
    


    <!-- http://purl.obolibrary.org/obo/GAZ_00011641 -->

    <owl:NamedIndividual rdf:about="http://purl.obolibrary.org/obo/GAZ_00011641">
        <obo:RO_0001025 rdf:resource="http://purl.obolibrary.org/obo/GAZ_00011619"/>
        <oboInOwl:hasOBONamespace>GAZ</oboInOwl:hasOBONamespace>
        <oboInOwl:id>GAZ:00011641</oboInOwl:id>
        <rdfs:label>Isla de Tortuga</rdfs:label>
    </owl:NamedIndividual>
    


    <!-- http://purl.obolibrary.org/obo/GAZ_00047116 -->

    <owl:NamedIndividual rdf:about="http://purl.obolibrary.org/obo/GAZ_00047116">
        <obo:RO_0001025 rdf:resource="http://purl.obolibrary.org/obo/GAZ_00011627"/>
        <obo:IAO_0000115>The largest island of the Nueva Esparta state in Venezuela, situated in the Caribbean Sea, off the northeastern coast of the country.</obo:IAO_0000115>
        <oboInOwl:hasOBONamespace>GAZ</oboInOwl:hasOBONamespace>
        <oboInOwl:id>GAZ:00047116</oboInOwl:id>
        <rdfs:label>Isla Margarita</rdfs:label>
    </owl:NamedIndividual>
    


    <!-- http://purl.obolibrary.org/obo/GAZ_00047117 -->

    <owl:NamedIndividual rdf:about="http://purl.obolibrary.org/obo/GAZ_00047117">
        <obo:RO_0001025 rdf:resource="http://purl.obolibrary.org/obo/GAZ_00011627"/>
        <oboInOwl:hasOBONamespace>GAZ</oboInOwl:hasOBONamespace>
        <oboInOwl:id>GAZ:00047117</oboInOwl:id>
        <rdfs:label>Isla Coche</rdfs:label>
    </owl:NamedIndividual>
    


    <!-- http://purl.obolibrary.org/obo/GAZ_00047118 -->

    <owl:NamedIndividual rdf:about="http://purl.obolibrary.org/obo/GAZ_00047118">
        <obo:RO_0001025 rdf:resource="http://purl.obolibrary.org/obo/GAZ_00011627"/>
        <oboInOwl:hasOBONamespace>GAZ</oboInOwl:hasOBONamespace>
        <oboInOwl:id>GAZ:00047118</oboInOwl:id>
        <rdfs:label>Isla Cubagua</rdfs:label>
    </owl:NamedIndividual>
    


    <!-- http://purl.obolibrary.org/obo/GAZ_00047130 -->

    <owl:NamedIndividual rdf:about="http://purl.obolibrary.org/obo/GAZ_00047130">
        <obo:IAO_0000115>The largest river in the world by volume, with a total river flow greater than the next top ten largest rivers flowing into the ocean combined.</obo:IAO_0000115>
        <oboInOwl:hasOBONamespace>GAZ</oboInOwl:hasOBONamespace>
        <oboInOwl:id>GAZ:00047130</oboInOwl:id>
        <rdfs:label>River Amazon</rdfs:label>
    </owl:NamedIndividual>
    


    <!-- http://purl.obolibrary.org/obo/GAZ_00047131 -->

    <owl:NamedIndividual rdf:about="http://purl.obolibrary.org/obo/GAZ_00047131">
        <obo:RO_0001025 rdf:resource="http://purl.obolibrary.org/obo/GAZ_00047130"/>
        <obo:IAO_0000115>A complex of broad river channels, islands, mangrove swamps, intertidal mudflats, brackish lagoons and marshes, palm swamps and seasonally flooded grassland and swamp forest. It extends from the SW tip of Ilha Grande de Gurupa 350 km NE to Ilha do Brique, Ilha Janauco, Ilha Caviana, Ilha Mexiana and Western Ilha Marajo.</obo:IAO_0000115>
        <oboInOwl:hasOBONamespace>GAZ</oboInOwl:hasOBONamespace>
        <oboInOwl:id>GAZ:00047131</oboInOwl:id>
        <rdfs:label>River Amazon Delta</rdfs:label>
    </owl:NamedIndividual>
    


    <!-- http://purl.obolibrary.org/obo/GAZ_00047132 -->

    <owl:NamedIndividual rdf:about="http://purl.obolibrary.org/obo/GAZ_00047132">
        <obo:RO_0001025 rdf:resource="http://purl.obolibrary.org/obo/GAZ_00047131"/>
        <obo:IAO_0000115>An island located at the mouth of the Amazon River in Brazil. It is part of the State of Para. It is the largest island to be completely surrounded by freshwater in the world. Although its northeast coastline faces the Atlantic Ocean, the outflow from the Amazon is so great that the sea at the mouth is quite unbriny for some distance from shore. The city of Belem lies to the south, across the southern fork (also called the Para River) of the river&apos;s mouth. The island sits almost directly on the equator.</obo:IAO_0000115>
        <oboInOwl:hasOBONamespace>GAZ</oboInOwl:hasOBONamespace>
        <oboInOwl:id>GAZ:00047132</oboInOwl:id>
        <rdfs:label>Ilha de Marajo</rdfs:label>
    </owl:NamedIndividual>
    


    <!-- http://purl.obolibrary.org/obo/GAZ_00049035 -->

    <owl:NamedIndividual rdf:about="http://purl.obolibrary.org/obo/GAZ_00049035">
        <obo:RO_0001025 rdf:resource="http://purl.obolibrary.org/obo/GAZ_00056519"/>
        <obo:IAO_0000115>An oligotrophic lake located in Neuquen, Argentina. Alumine Lake is fed by the outflow of Lake Moquehue. Pertenece a la cuenca del rio Negro, al que desagua a traves de los rios Alumine, Collon Cura y Limay.</obo:IAO_0000115>
        <oboInOwl:hasOBONamespace>GAZ</oboInOwl:hasOBONamespace>
        <oboInOwl:id>GAZ:00049035</oboInOwl:id>
        <rdfs:label>Lago Alumine</rdfs:label>
    </owl:NamedIndividual>
    


    <!-- http://purl.obolibrary.org/obo/GAZ_00049220 -->

    <owl:NamedIndividual rdf:about="http://purl.obolibrary.org/obo/GAZ_00049220">
        <obo:RO_0001025 rdf:resource="http://purl.obolibrary.org/obo/GAZ_00002931"/>
        <obo:IAO_0000115>A river. A tributary of the Orinoco River, entering 4 miles from the Atlantic Ocean. It originates in Guyana, flowing for approximately 210 miles before entering Venezuela about 50 miles from its mouth.</obo:IAO_0000115>
        <oboInOwl:hasOBONamespace>GAZ</oboInOwl:hasOBONamespace>
        <oboInOwl:id>GAZ:00049220</oboInOwl:id>
        <rdfs:label>Barima River</rdfs:label>
    </owl:NamedIndividual>
    


    <!-- http://purl.obolibrary.org/obo/GAZ_00049221 -->

    <owl:NamedIndividual rdf:about="http://purl.obolibrary.org/obo/GAZ_00049221">
        <obo:RO_0001025 rdf:resource="http://purl.obolibrary.org/obo/GAZ_00049220"/>
        <oboInOwl:hasOBONamespace>GAZ</oboInOwl:hasOBONamespace>
        <oboInOwl:id>GAZ:00049221</oboInOwl:id>
        <rdfs:label>Barima River delta</rdfs:label>
    </owl:NamedIndividual>
    


    <!-- http://purl.obolibrary.org/obo/GAZ_00049222 -->

    <owl:NamedIndividual rdf:about="http://purl.obolibrary.org/obo/GAZ_00049222">
        <obo:RO_0001025 rdf:resource="http://purl.obolibrary.org/obo/GAZ_00049221"/>
        <obo:IAO_0000115>An island split between Venezuela and Guyana.</obo:IAO_0000115>
        <oboInOwl:hasOBONamespace>GAZ</oboInOwl:hasOBONamespace>
        <oboInOwl:id>GAZ:00049222</oboInOwl:id>
        <rdfs:label>Corocoro Island</rdfs:label>
    </owl:NamedIndividual>
    


    <!-- http://purl.obolibrary.org/obo/GAZ_00049223 -->

    <owl:NamedIndividual rdf:about="http://purl.obolibrary.org/obo/GAZ_00049223">
        <obo:IAO_0000115>The largest left tributary of the Amazon and the largest blackwater river in the world. It has its sources along the watershed between the Orinoco and the Amazon basins, and also connects with the Orinoco by way of the Casiquiare canal. In Colombia, where their sources are, it is called the Guainia River. Its main affluent is Vaupes, which disputes with the headwaters of the Guaviare branch of the Orinoco, the drainage of the eastern slope of the Andes of Colombia. The Rio Negro flows into the Rio Solimoes to form the Amazon River near Manaus, Brazil.</obo:IAO_0000115>
        <oboInOwl:hasOBONamespace>GAZ</oboInOwl:hasOBONamespace>
        <oboInOwl:id>GAZ:00049223</oboInOwl:id>
        <rdfs:label>Rio Negro</rdfs:label>
    </owl:NamedIndividual>
    


    <!-- http://purl.obolibrary.org/obo/GAZ_00049224 -->

    <owl:NamedIndividual rdf:about="http://purl.obolibrary.org/obo/GAZ_00049224">
        <obo:RO_0001025 rdf:resource="http://purl.obolibrary.org/obo/GAZ_00049223"/>
        <obo:IAO_0000115>An island split between Brazil and Colombia.</obo:IAO_0000115>
        <oboInOwl:hasOBONamespace>GAZ</oboInOwl:hasOBONamespace>
        <oboInOwl:id>GAZ:00049224</oboInOwl:id>
        <rdfs:label>San Jose Island</rdfs:label>
    </owl:NamedIndividual>
    


    <!-- http://purl.obolibrary.org/obo/GAZ_00051232 -->

    <owl:NamedIndividual rdf:about="http://purl.obolibrary.org/obo/GAZ_00051232">
        <obo:IAO_0000115>An area of inland drainage lying in the central Andes, occupying parts of Chile, Argentina, Bolivia, Peru and Ecuador. Its height averages about 3,300 m.</obo:IAO_0000115>
        <oboInOwl:hasOBONamespace>GAZ</oboInOwl:hasOBONamespace>
        <oboInOwl:id>GAZ:00051232</oboInOwl:id>
        <rdfs:label>Altiplano Basin</rdfs:label>
    </owl:NamedIndividual>
    


    <!-- http://purl.obolibrary.org/obo/GAZ_00051234 -->

    <owl:NamedIndividual rdf:about="http://purl.obolibrary.org/obo/GAZ_00051234">
        <obo:RO_0001025 rdf:resource="http://purl.obolibrary.org/obo/GAZ_00011615"/>
        <obo:IAO_0000115>An artificial lake formed by a dam on the Caroni River.</obo:IAO_0000115>
        <oboInOwl:hasOBONamespace>GAZ</oboInOwl:hasOBONamespace>
        <oboInOwl:id>GAZ:00051234</oboInOwl:id>
        <rdfs:label>Lake Guri</rdfs:label>
    </owl:NamedIndividual>
    


    <!-- http://purl.obolibrary.org/obo/GAZ_00051544 -->

    <owl:NamedIndividual rdf:about="http://purl.obolibrary.org/obo/GAZ_00051544">
        <obo:RO_0001025 rdf:resource="http://purl.obolibrary.org/obo/GAZ_00011631"/>
        <oboInOwl:hasOBONamespace>GAZ</oboInOwl:hasOBONamespace>
        <oboInOwl:id>GAZ:00051544</oboInOwl:id>
        <rdfs:label>Isla Pico</rdfs:label>
    </owl:NamedIndividual>
    


    <!-- http://purl.obolibrary.org/obo/GAZ_00051546 -->

    <owl:NamedIndividual rdf:about="http://purl.obolibrary.org/obo/GAZ_00051546">
        <obo:RO_0001025 rdf:resource="http://purl.obolibrary.org/obo/GAZ_00011619"/>
        <obo:RO_0001025 rdf:resource="http://purl.obolibrary.org/obo/GAZ_00011631"/>
        <obo:IAO_0000115>An island off the coast of Venezuela, north of Caracas.</obo:IAO_0000115>
        <oboInOwl:hasOBONamespace>GAZ</oboInOwl:hasOBONamespace>
        <oboInOwl:id>GAZ:00051546</oboInOwl:id>
        <rdfs:label>Isla La Orquilla</rdfs:label>
    </owl:NamedIndividual>
    


    <!-- http://purl.obolibrary.org/obo/GAZ_00051547 -->

    <owl:NamedIndividual rdf:about="http://purl.obolibrary.org/obo/GAZ_00051547">
        <obo:RO_0001025 rdf:resource="http://purl.obolibrary.org/obo/GAZ_00011631"/>
        <oboInOwl:hasOBONamespace>GAZ</oboInOwl:hasOBONamespace>
        <oboInOwl:id>GAZ:00051547</oboInOwl:id>
        <rdfs:label>Isla Chiquito</rdfs:label>
    </owl:NamedIndividual>
    


    <!-- http://purl.obolibrary.org/obo/GAZ_00051548 -->

    <owl:NamedIndividual rdf:about="http://purl.obolibrary.org/obo/GAZ_00051548">
        <obo:RO_0001025 rdf:resource="http://purl.obolibrary.org/obo/GAZ_00011631"/>
        <oboInOwl:hasOBONamespace>GAZ</oboInOwl:hasOBONamespace>
        <oboInOwl:id>GAZ:00051548</oboInOwl:id>
        <rdfs:label>Isla Fondeadero</rdfs:label>
    </owl:NamedIndividual>
    


    <!-- http://purl.obolibrary.org/obo/GAZ_00051549 -->

    <owl:NamedIndividual rdf:about="http://purl.obolibrary.org/obo/GAZ_00051549">
        <obo:RO_0001025 rdf:resource="http://purl.obolibrary.org/obo/GAZ_00011631"/>
        <oboInOwl:hasOBONamespace>GAZ</oboInOwl:hasOBONamespace>
        <oboInOwl:id>GAZ:00051549</oboInOwl:id>
        <rdfs:label>Isla Los Morochos</rdfs:label>
    </owl:NamedIndividual>
    


    <!-- http://purl.obolibrary.org/obo/GAZ_00051550 -->

    <owl:NamedIndividual rdf:about="http://purl.obolibrary.org/obo/GAZ_00051550">
        <obo:RO_0001025 rdf:resource="http://purl.obolibrary.org/obo/GAZ_00011631"/>
        <oboInOwl:hasOBONamespace>GAZ</oboInOwl:hasOBONamespace>
        <oboInOwl:id>GAZ:00051550</oboInOwl:id>
        <rdfs:label>Isla Grueso</rdfs:label>
    </owl:NamedIndividual>
    


    <!-- http://purl.obolibrary.org/obo/GAZ_00051567 -->

    <owl:NamedIndividual rdf:about="http://purl.obolibrary.org/obo/GAZ_00051567">
        <obo:RO_0001025 rdf:resource="http://purl.obolibrary.org/obo/GAZ_00011635"/>
        <oboInOwl:hasOBONamespace>GAZ</oboInOwl:hasOBONamespace>
        <oboInOwl:id>GAZ:00051567</oboInOwl:id>
        <rdfs:label>Nabobo Island</rdfs:label>
    </owl:NamedIndividual>
    


    <!-- http://purl.obolibrary.org/obo/GAZ_00051568 -->

    <owl:NamedIndividual rdf:about="http://purl.obolibrary.org/obo/GAZ_00051568">
        <obo:RO_0001025 rdf:resource="http://purl.obolibrary.org/obo/GAZ_00011635"/>
        <oboInOwl:hasOBONamespace>GAZ</oboInOwl:hasOBONamespace>
        <oboInOwl:id>GAZ:00051568</oboInOwl:id>
        <rdfs:label>Guacaraida Island</rdfs:label>
    </owl:NamedIndividual>
    


    <!-- http://purl.obolibrary.org/obo/GAZ_00051569 -->

    <owl:NamedIndividual rdf:about="http://purl.obolibrary.org/obo/GAZ_00051569">
        <obo:RO_0001025 rdf:resource="http://purl.obolibrary.org/obo/GAZ_00011635"/>
        <oboInOwl:hasOBONamespace>GAZ</oboInOwl:hasOBONamespace>
        <oboInOwl:id>GAZ:00051569</oboInOwl:id>
        <rdfs:label>La Peche Island</rdfs:label>
    </owl:NamedIndividual>
    


    <!-- http://purl.obolibrary.org/obo/GAZ_00051570 -->

    <owl:NamedIndividual rdf:about="http://purl.obolibrary.org/obo/GAZ_00051570">
        <obo:RO_0001025 rdf:resource="http://purl.obolibrary.org/obo/GAZ_00011635"/>
        <oboInOwl:hasOBONamespace>GAZ</oboInOwl:hasOBONamespace>
        <oboInOwl:id>GAZ:00051570</oboInOwl:id>
        <rdfs:label>Macarare Island</rdfs:label>
    </owl:NamedIndividual>
    


    <!-- http://purl.obolibrary.org/obo/GAZ_00051571 -->

    <owl:NamedIndividual rdf:about="http://purl.obolibrary.org/obo/GAZ_00051571">
        <obo:RO_0001025 rdf:resource="http://purl.obolibrary.org/obo/GAZ_00011635"/>
        <oboInOwl:hasOBONamespace>GAZ</oboInOwl:hasOBONamespace>
        <oboInOwl:id>GAZ:00051571</oboInOwl:id>
        <rdfs:label>Guairiare Island</rdfs:label>
    </owl:NamedIndividual>
    


    <!-- http://purl.obolibrary.org/obo/GAZ_00051572 -->

    <owl:NamedIndividual rdf:about="http://purl.obolibrary.org/obo/GAZ_00051572">
        <obo:RO_0001025 rdf:resource="http://purl.obolibrary.org/obo/GAZ_00011635"/>
        <oboInOwl:hasOBONamespace>GAZ</oboInOwl:hasOBONamespace>
        <oboInOwl:id>GAZ:00051572</oboInOwl:id>
        <rdfs:label>La Balandra Island</rdfs:label>
    </owl:NamedIndividual>
    


    <!-- http://purl.obolibrary.org/obo/GAZ_00051573 -->

    <owl:NamedIndividual rdf:about="http://purl.obolibrary.org/obo/GAZ_00051573">
        <obo:RO_0001025 rdf:resource="http://purl.obolibrary.org/obo/GAZ_00011635"/>
        <oboInOwl:hasOBONamespace>GAZ</oboInOwl:hasOBONamespace>
        <oboInOwl:id>GAZ:00051573</oboInOwl:id>
        <rdfs:label>Chepere Island</rdfs:label>
    </owl:NamedIndividual>
    


    <!-- http://purl.obolibrary.org/obo/GAZ_00051574 -->

    <owl:NamedIndividual rdf:about="http://purl.obolibrary.org/obo/GAZ_00051574">
        <obo:RO_0001025 rdf:resource="http://purl.obolibrary.org/obo/GAZ_00011635"/>
        <oboInOwl:hasOBONamespace>GAZ</oboInOwl:hasOBONamespace>
        <oboInOwl:id>GAZ:00051574</oboInOwl:id>
        <rdfs:label>Puerto Real Island</rdfs:label>
    </owl:NamedIndividual>
    


    <!-- http://purl.obolibrary.org/obo/GAZ_00051575 -->

    <owl:NamedIndividual rdf:about="http://purl.obolibrary.org/obo/GAZ_00051575">
        <obo:RO_0001025 rdf:resource="http://purl.obolibrary.org/obo/GAZ_00011635"/>
        <oboInOwl:hasOBONamespace>GAZ</oboInOwl:hasOBONamespace>
        <oboInOwl:id>GAZ:00051575</oboInOwl:id>
        <rdfs:label>Guacaraida Island</rdfs:label>
    </owl:NamedIndividual>
    


    <!-- http://purl.obolibrary.org/obo/GAZ_00051576 -->

    <owl:NamedIndividual rdf:about="http://purl.obolibrary.org/obo/GAZ_00051576">
        <obo:RO_0001025 rdf:resource="http://purl.obolibrary.org/obo/GAZ_00011635"/>
        <oboInOwl:hasOBONamespace>GAZ</oboInOwl:hasOBONamespace>
        <oboInOwl:id>GAZ:00051576</oboInOwl:id>
        <rdfs:label>Cominoto Island</rdfs:label>
    </owl:NamedIndividual>
    


    <!-- http://purl.obolibrary.org/obo/GAZ_00051577 -->

    <owl:NamedIndividual rdf:about="http://purl.obolibrary.org/obo/GAZ_00051577">
        <obo:RO_0001025 rdf:resource="http://purl.obolibrary.org/obo/GAZ_00011635"/>
        <obo:IAO_0000115>A 3 m high rock located 8 km N of the Los Frailes Archipelago.</obo:IAO_0000115>
        <oboInOwl:hasOBONamespace>GAZ</oboInOwl:hasOBONamespace>
        <oboInOwl:id>GAZ:00051577</oboInOwl:id>
        <rdfs:label>Roca del Norte</rdfs:label>
    </owl:NamedIndividual>
    


    <!-- http://purl.obolibrary.org/obo/GAZ_00051743 -->

    <owl:NamedIndividual rdf:about="http://purl.obolibrary.org/obo/GAZ_00051743">
        <obo:RO_0001025 rdf:resource="http://purl.obolibrary.org/obo/GAZ_00011634"/>
        <obo:IAO_0000115>An atoll. The western group of Las Aves Archipelago, with Isla Maceta, a large mangrove-covered cay in the south.</obo:IAO_0000115>
        <oboInOwl:hasOBONamespace>GAZ</oboInOwl:hasOBONamespace>
        <oboInOwl:id>GAZ:00051743</oboInOwl:id>
        <rdfs:label>Aves de Sotavento</rdfs:label>
    </owl:NamedIndividual>
    


    <!-- http://purl.obolibrary.org/obo/GAZ_00051744 -->

    <owl:NamedIndividual rdf:about="http://purl.obolibrary.org/obo/GAZ_00051744">
        <obo:RO_0001025 rdf:resource="http://purl.obolibrary.org/obo/GAZ_00011634"/>
        <obo:IAO_0000115>An atoll. The eastern group of Las Aves Archipelago, with a fringing reef of 8 km of diameter and with three cays in the southwest.</obo:IAO_0000115>
        <oboInOwl:hasOBONamespace>GAZ</oboInOwl:hasOBONamespace>
        <oboInOwl:id>GAZ:00051744</oboInOwl:id>
        <rdfs:label>Aves de Barlovento</rdfs:label>
    </owl:NamedIndividual>
    


    <!-- http://purl.obolibrary.org/obo/GAZ_00051748 -->

    <owl:NamedIndividual rdf:about="http://purl.obolibrary.org/obo/GAZ_00051748">
        <obo:RO_0001025 rdf:resource="http://purl.obolibrary.org/obo/GAZ_00011633"/>
        <oboInOwl:hasOBONamespace>GAZ</oboInOwl:hasOBONamespace>
        <oboInOwl:id>GAZ:00051748</oboInOwl:id>
        <rdfs:label>Isla Este</rdfs:label>
    </owl:NamedIndividual>
    


    <!-- http://purl.obolibrary.org/obo/GAZ_00051749 -->

    <owl:NamedIndividual rdf:about="http://purl.obolibrary.org/obo/GAZ_00051749">
        <obo:RO_0001025 rdf:resource="http://purl.obolibrary.org/obo/GAZ_00011633"/>
        <oboInOwl:hasOBONamespace>GAZ</oboInOwl:hasOBONamespace>
        <oboInOwl:id>GAZ:00051749</oboInOwl:id>
        <rdfs:label>Isla Sur</rdfs:label>
    </owl:NamedIndividual>
    


    <!-- http://purl.obolibrary.org/obo/GAZ_00051750 -->

    <owl:NamedIndividual rdf:about="http://purl.obolibrary.org/obo/GAZ_00051750">
        <obo:RO_0001025 rdf:resource="http://purl.obolibrary.org/obo/GAZ_00011633"/>
        <oboInOwl:hasOBONamespace>GAZ</oboInOwl:hasOBONamespace>
        <oboInOwl:id>GAZ:00051750</oboInOwl:id>
        <rdfs:label>Isla Norte</rdfs:label>
    </owl:NamedIndividual>
    


    <!-- http://purl.obolibrary.org/obo/GAZ_00051751 -->

    <owl:NamedIndividual rdf:about="http://purl.obolibrary.org/obo/GAZ_00051751">
        <obo:RO_0001025 rdf:resource="http://purl.obolibrary.org/obo/GAZ_00011638"/>
        <oboInOwl:hasOBONamespace>GAZ</oboInOwl:hasOBONamespace>
        <oboInOwl:id>GAZ:00051751</oboInOwl:id>
        <rdfs:label>El Gran Roque</rdfs:label>
    </owl:NamedIndividual>
    


    <!-- http://purl.obolibrary.org/obo/GAZ_00051752 -->

    <owl:NamedIndividual rdf:about="http://purl.obolibrary.org/obo/GAZ_00051752">
        <obo:RO_0001025 rdf:resource="http://purl.obolibrary.org/obo/GAZ_00011638"/>
        <oboInOwl:hasOBONamespace>GAZ</oboInOwl:hasOBONamespace>
        <oboInOwl:id>GAZ:00051752</oboInOwl:id>
        <rdfs:label>Isla Crasqui</rdfs:label>
    </owl:NamedIndividual>
    


    <!-- http://purl.obolibrary.org/obo/GAZ_00051753 -->

    <owl:NamedIndividual rdf:about="http://purl.obolibrary.org/obo/GAZ_00051753">
        <obo:RO_0001025 rdf:resource="http://purl.obolibrary.org/obo/GAZ_00011638"/>
        <oboInOwl:hasOBONamespace>GAZ</oboInOwl:hasOBONamespace>
        <oboInOwl:id>GAZ:00051753</oboInOwl:id>
        <rdfs:label>Isla Francisqui</rdfs:label>
    </owl:NamedIndividual>
    


    <!-- http://purl.obolibrary.org/obo/GAZ_00051754 -->

    <owl:NamedIndividual rdf:about="http://purl.obolibrary.org/obo/GAZ_00051754">
        <obo:RO_0001025 rdf:resource="http://purl.obolibrary.org/obo/GAZ_00011638"/>
        <oboInOwl:hasOBONamespace>GAZ</oboInOwl:hasOBONamespace>
        <oboInOwl:id>GAZ:00051754</oboInOwl:id>
        <rdfs:label>Isla Nordisqui</rdfs:label>
    </owl:NamedIndividual>
    


    <!-- http://purl.obolibrary.org/obo/GAZ_00051755 -->

    <owl:NamedIndividual rdf:about="http://purl.obolibrary.org/obo/GAZ_00051755">
        <obo:RO_0001025 rdf:resource="http://purl.obolibrary.org/obo/GAZ_00011638"/>
        <oboInOwl:hasOBONamespace>GAZ</oboInOwl:hasOBONamespace>
        <oboInOwl:id>GAZ:00051755</oboInOwl:id>
        <rdfs:label>Isla Madrisqui</rdfs:label>
    </owl:NamedIndividual>
    


    <!-- http://purl.obolibrary.org/obo/GAZ_00051756 -->

    <owl:NamedIndividual rdf:about="http://purl.obolibrary.org/obo/GAZ_00051756">
        <obo:RO_0001025 rdf:resource="http://purl.obolibrary.org/obo/GAZ_00011638"/>
        <oboInOwl:hasOBONamespace>GAZ</oboInOwl:hasOBONamespace>
        <oboInOwl:id>GAZ:00051756</oboInOwl:id>
        <rdfs:label>Isla Sarky</rdfs:label>
    </owl:NamedIndividual>
    


    <!-- http://purl.obolibrary.org/obo/GAZ_00051757 -->

    <owl:NamedIndividual rdf:about="http://purl.obolibrary.org/obo/GAZ_00051757">
        <obo:RO_0001025 rdf:resource="http://purl.obolibrary.org/obo/GAZ_00011638"/>
        <oboInOwl:hasOBONamespace>GAZ</oboInOwl:hasOBONamespace>
        <oboInOwl:id>GAZ:00051757</oboInOwl:id>
        <rdfs:label>Isla Noronky</rdfs:label>
    </owl:NamedIndividual>
    


    <!-- http://purl.obolibrary.org/obo/GAZ_00051758 -->

    <owl:NamedIndividual rdf:about="http://purl.obolibrary.org/obo/GAZ_00051758">
        <obo:RO_0001025 rdf:resource="http://purl.obolibrary.org/obo/GAZ_00011638"/>
        <oboInOwl:hasOBONamespace>GAZ</oboInOwl:hasOBONamespace>
        <oboInOwl:id>GAZ:00051758</oboInOwl:id>
        <rdfs:label>Isla Carenero</rdfs:label>
    </owl:NamedIndividual>
    


    <!-- http://purl.obolibrary.org/obo/GAZ_00051759 -->

    <owl:NamedIndividual rdf:about="http://purl.obolibrary.org/obo/GAZ_00051759">
        <obo:RO_0001025 rdf:resource="http://purl.obolibrary.org/obo/GAZ_00011638"/>
        <oboInOwl:hasOBONamespace>GAZ</oboInOwl:hasOBONamespace>
        <oboInOwl:id>GAZ:00051759</oboInOwl:id>
        <rdfs:label>Isla Espenky</rdfs:label>
    </owl:NamedIndividual>
    


    <!-- http://purl.obolibrary.org/obo/GAZ_00056247 -->

    <owl:NamedIndividual rdf:about="http://purl.obolibrary.org/obo/GAZ_00056247">
        <obo:RO_0001025 rdf:resource="http://purl.obolibrary.org/obo/GAZ_00056262"/>
        <obo:IAO_0000115>One of three branches of the Andes Mountains in Colombia that divide at the Node of Pasto, extending from south to north from Narino to the Node of Paramillo in Cordoba. The western part of the mountain range belongs mainly to the Pacific region, with the San Juan River standing out, while the eastern part belongs mainly to the Cauca River basin. The northern part and northwestern part belong to the Atlantic Slope, with the Atrato and Sinu rivers standing out. The Cordillera Occidental is separted from the coastal Baudo Mountains by the Atrato River.</obo:IAO_0000115>
        <oboInOwl:hasOBONamespace>GAZ</oboInOwl:hasOBONamespace>
        <oboInOwl:id>GAZ:00056247</oboInOwl:id>
        <rdfs:label>Cordillera Occidental of Colombia</rdfs:label>
    </owl:NamedIndividual>
    


    <!-- http://purl.obolibrary.org/obo/GAZ_00056248 -->

    <owl:NamedIndividual rdf:about="http://purl.obolibrary.org/obo/GAZ_00056248">
        <obo:RO_0001025 rdf:resource="http://purl.obolibrary.org/obo/GAZ_00056262"/>
        <obo:IAO_0000115>A mountain range characterized by volcanic activity, making up the natural border with Chile and starting in the north with Jucuri and ending in the south at the Licancabur volcano, which is on the southern border of Bolivia. The range consists of three sections.</obo:IAO_0000115>
        <oboInOwl:hasOBONamespace>GAZ</oboInOwl:hasOBONamespace>
        <oboInOwl:id>GAZ:00056248</oboInOwl:id>
        <rdfs:label>Cordillera Occidental of Bolivia</rdfs:label>
    </owl:NamedIndividual>
    


    <!-- http://purl.obolibrary.org/obo/GAZ_00056249 -->

    <owl:NamedIndividual rdf:about="http://purl.obolibrary.org/obo/GAZ_00056249">
        <obo:RO_0001025 rdf:resource="http://purl.obolibrary.org/obo/GAZ_00056248"/>
        <oboInOwl:hasOBONamespace>GAZ</oboInOwl:hasOBONamespace>
        <oboInOwl:id>GAZ:00056249</oboInOwl:id>
        <rdfs:label>Cordillera Occidental of Bolivia, Meridional</rdfs:label>
    </owl:NamedIndividual>
    


    <!-- http://purl.obolibrary.org/obo/GAZ_00056250 -->

    <owl:NamedIndividual rdf:about="http://purl.obolibrary.org/obo/GAZ_00056250">
        <obo:RO_0001025 rdf:resource="http://purl.obolibrary.org/obo/GAZ_00056248"/>
        <obo:IAO_0000115>That part of the Cordillera Occidental of Bolivia that is situated between Uyuni and Coipasa. Its most prominent summit is the Ollague volcano on the border with Chile.</obo:IAO_0000115>
        <oboInOwl:hasOBONamespace>GAZ</oboInOwl:hasOBONamespace>
        <oboInOwl:id>GAZ:00056250</oboInOwl:id>
        <rdfs:label>Cordillera Occidental of Bolivia, Central</rdfs:label>
    </owl:NamedIndividual>
    


    <!-- http://purl.obolibrary.org/obo/GAZ_00056251 -->

    <owl:NamedIndividual rdf:about="http://purl.obolibrary.org/obo/GAZ_00056251">
        <obo:RO_0001025 rdf:resource="http://purl.obolibrary.org/obo/GAZ_00056248"/>
        <oboInOwl:hasOBONamespace>GAZ</oboInOwl:hasOBONamespace>
        <oboInOwl:id>GAZ:00056251</oboInOwl:id>
        <rdfs:label>Cordillera Occidental of Bolivia, Septentrional</rdfs:label>
    </owl:NamedIndividual>
    


    <!-- http://purl.obolibrary.org/obo/GAZ_00056252 -->

    <owl:NamedIndividual rdf:about="http://purl.obolibrary.org/obo/GAZ_00056252">
        <obo:RO_0001025 rdf:resource="http://purl.obolibrary.org/obo/GAZ_00056262"/>
        <obo:IAO_0000115>One of two main ranges in the Andes in Ecuador, the other being the Cordillera Central. It spans the whole country from north to south.</obo:IAO_0000115>
        <oboInOwl:hasOBONamespace>GAZ</oboInOwl:hasOBONamespace>
        <oboInOwl:id>GAZ:00056252</oboInOwl:id>
        <rdfs:label>Cordillera Occidental of Ecuador</rdfs:label>
    </owl:NamedIndividual>
    


    <!-- http://purl.obolibrary.org/obo/GAZ_00056254 -->

    <owl:NamedIndividual rdf:about="http://purl.obolibrary.org/obo/GAZ_00056254">
        <obo:RO_0001025 rdf:resource="http://purl.obolibrary.org/obo/GAZ_00056288"/>
        <obo:IAO_0000115>One of the three branches of ridges in the Andes Mountains that split in southern Colombia towards the north up to the Montes de Maria. It extends from the Nudo de Almaguer, or the &quot;Colombian Mountain Mass&quot; in Cauca, located in southern Colombia, to the Serrania of San Lucas in Bolivar to the north. The range is bounded by the Cauca and Magdalena river valleys to the west and east, respectively.</obo:IAO_0000115>
        <oboInOwl:hasOBONamespace>GAZ</oboInOwl:hasOBONamespace>
        <oboInOwl:id>GAZ:00056254</oboInOwl:id>
        <rdfs:label>Cordillera Central of Colombia</rdfs:label>
    </owl:NamedIndividual>
    


    <!-- http://purl.obolibrary.org/obo/GAZ_00056259 -->

    <owl:NamedIndividual rdf:about="http://purl.obolibrary.org/obo/GAZ_00056259">
        <rdf:type rdf:resource="http://purl.obolibrary.org/obo/ENVO_00000032"/>
        <obo:RO_0001025 rdf:resource="http://purl.obolibrary.org/obo/GAZ_00002931"/>
        <obo:IAO_0000115>A gulf of the Caribbean Sea bounded by the Venezuelan states of Zulia and Falcon and the Colombian Department (State) of Guajira. A 54 km strait connects it with Lake Maracaibo to the south. The Gulf is located in the north of South America, between the peninsulas of Paraguana of the Falcon State in Venezuela and Guajira&apos;s in Colombia.</obo:IAO_0000115>
        <oboInOwl:hasOBONamespace>GAZ</oboInOwl:hasOBONamespace>
        <oboInOwl:id>GAZ:00056259</oboInOwl:id>
        <rdfs:label>Gulf of Venezuela</rdfs:label>
    </owl:NamedIndividual>
    


    <!-- http://purl.obolibrary.org/obo/GAZ_00056260 -->

    <owl:NamedIndividual rdf:about="http://purl.obolibrary.org/obo/GAZ_00056260">
        <obo:RO_0001025 rdf:resource="http://purl.obolibrary.org/obo/GAZ_00056263"/>
        <obo:IAO_0000115>One of three main mountain ranges that divides the Cordillera in the Andes Mountains of Colombia. It extends from southeast to northeast from the Nudo de Almaguer, or the &quot;Colombia Mountain Mass&quot; in Cauca to the Perija Mountains in La Guajira. The western part of the Cordillera Oriental belongs to the Magdalena River basin, while the eastern part includes the river basins of the Amazon River, Orinoco, and Catatumbo.</obo:IAO_0000115>
        <oboInOwl:hasOBONamespace>GAZ</oboInOwl:hasOBONamespace>
        <oboInOwl:id>GAZ:00056260</oboInOwl:id>
        <rdfs:label>Cordillera Oriental of Colombia</rdfs:label>
    </owl:NamedIndividual>
    


    <!-- http://purl.obolibrary.org/obo/GAZ_00056261 -->

    <owl:NamedIndividual rdf:about="http://purl.obolibrary.org/obo/GAZ_00056261">
        <obo:RO_0001025 rdf:resource="http://purl.obolibrary.org/obo/GAZ_00056263"/>
        <obo:IAO_0000115>A mountain range.</obo:IAO_0000115>
        <oboInOwl:hasOBONamespace>GAZ</oboInOwl:hasOBONamespace>
        <oboInOwl:id>GAZ:00056261</oboInOwl:id>
        <rdfs:label>Cordillera Oriental of Peru</rdfs:label>
    </owl:NamedIndividual>
    


    <!-- http://purl.obolibrary.org/obo/GAZ_00056262 -->

    <owl:NamedIndividual rdf:about="http://purl.obolibrary.org/obo/GAZ_00056262">
        <obo:IAO_0000115>The W of the two main subranges of the Andes.</obo:IAO_0000115>
        <oboInOwl:hasOBONamespace>GAZ</oboInOwl:hasOBONamespace>
        <oboInOwl:id>GAZ:00056262</oboInOwl:id>
        <rdfs:label>Cordillera Occidental</rdfs:label>
    </owl:NamedIndividual>
    


    <!-- http://purl.obolibrary.org/obo/GAZ_00056263 -->

    <owl:NamedIndividual rdf:about="http://purl.obolibrary.org/obo/GAZ_00056263">
        <obo:IAO_0000115>The E of the two main subranges of the Andes.</obo:IAO_0000115>
        <oboInOwl:hasOBONamespace>GAZ</oboInOwl:hasOBONamespace>
        <oboInOwl:id>GAZ:00056263</oboInOwl:id>
        <rdfs:label>Cordillera Oriental</rdfs:label>
    </owl:NamedIndividual>
    


    <!-- http://purl.obolibrary.org/obo/GAZ_00056265 -->

    <owl:NamedIndividual rdf:about="http://purl.obolibrary.org/obo/GAZ_00056265">
        <obo:RO_0001025 rdf:resource="http://purl.obolibrary.org/obo/GAZ_00002931"/>
        <obo:IAO_0000115>A mountain range that runs along the central and eastern portions of Venezuela&apos;s northern coast. The range is a northeastern extension of the Andes Mountains, and is also known as the Maritime Andes. The Coastal Range actually consists of two parallel ranges, which run east and west along the coast of the Caribbean Sea. The Cojedes River separates the western end of Coastal Range from the Cordillera de Merida to the southeast. The range is divided into eastern and western sections by the wide bay between Cape Codera and Cumana. In eastern section of the range, the parallel ranges are known as the Serrania del Litoral, which runs along the Caribbean coast, and the Serrania del Interior. The valley between these two ranges, which includes Lake Valencia, the valleys of Caracas, and the Tuy River at its eastern end, is the most densely peopled part of Venezuela. Caracas lies in a valley between two branches of the Serrania del Litoral: the Avila to the north, and smaller hills to the south. Both the littoral and interior ranges reappear between Cumana and the Gulf of Paria to form the eastern section of the cordillera. The Littoral range forms the Araya Peninsula to the west and the Paria Peninsula to the west, and extends across the straits known as the Dragon&apos;s Mouths to form the Northern Range of the island of Trinidad.</obo:IAO_0000115>
        <oboInOwl:hasOBONamespace>GAZ</oboInOwl:hasOBONamespace>
        <oboInOwl:id>GAZ:00056265</oboInOwl:id>
        <rdfs:label>Cordillera de la Costa</rdfs:label>
    </owl:NamedIndividual>
    


    <!-- http://purl.obolibrary.org/obo/GAZ_00056266 -->

    <owl:NamedIndividual rdf:about="http://purl.obolibrary.org/obo/GAZ_00056266">
        <obo:RO_0001025 rdf:resource="http://purl.obolibrary.org/obo/GAZ_00056254"/>
        <obo:RO_0001025 rdf:resource="http://purl.obolibrary.org/obo/GAZ_00136448"/>
        <obo:IAO_0000115>A stratovolcano that is truncated by a 2.5 x 3 km caldera containing a Holocene rhyodacitic lava-dome complex. A crescent-shaped lake, Laguna Verde, occupies the NW side of the caldera. Nearly a dozen lava domes are present, the latest of which were formed about 3600 years ago and have active fumaroles. Azufral rocks are more silicic than those of nearby Colombian volcanoes; an apron of rhyodacitic pyroclastic-flow deposits rings the volcano. The last known eruption of Volcan Azufral took place about 1000 years ago.</obo:IAO_0000115>
        <oboInOwl:hasOBONamespace>GAZ</oboInOwl:hasOBONamespace>
        <oboInOwl:id>GAZ:00056266</oboInOwl:id>
        <rdfs:label>Volcan Azufral</rdfs:label>
    </owl:NamedIndividual>
    


    <!-- http://purl.obolibrary.org/obo/GAZ_00056267 -->

    <owl:NamedIndividual rdf:about="http://purl.obolibrary.org/obo/GAZ_00056267">
        <obo:RO_0001025 rdf:resource="http://purl.obolibrary.org/obo/GAZ_00056266"/>
        <obo:IAO_0000115>A caldera lake that occupies the NW side of the Azufral caldera.</obo:IAO_0000115>
        <oboInOwl:hasOBONamespace>GAZ</oboInOwl:hasOBONamespace>
        <oboInOwl:id>GAZ:00056267</oboInOwl:id>
        <rdfs:label>Laguna Verde</rdfs:label>
    </owl:NamedIndividual>
    


    <!-- http://purl.obolibrary.org/obo/GAZ_00056268 -->

    <owl:NamedIndividual rdf:about="http://purl.obolibrary.org/obo/GAZ_00056268">
        <obo:RO_0001025 rdf:resource="http://purl.obolibrary.org/obo/GAZ_00056254"/>
        <obo:RO_0001025 rdf:resource="http://purl.obolibrary.org/obo/GAZ_00136448"/>
        <obo:IAO_0000115>A relatively low dominantly dacitic lava-dome complex north of Nevado del Ruiz volcano that was constructed within the Pleistocene Quebrada Seca caldera. A series of moderate plinian eruptions during the Holocene has been accompanied by pyroclastic flows and lava dome growth.</obo:IAO_0000115>
        <oboInOwl:hasOBONamespace>GAZ</oboInOwl:hasOBONamespace>
        <oboInOwl:id>GAZ:00056268</oboInOwl:id>
        <rdfs:label>Cerro Bravo</rdfs:label>
    </owl:NamedIndividual>
    


    <!-- http://purl.obolibrary.org/obo/GAZ_00056269 -->

    <owl:NamedIndividual rdf:about="http://purl.obolibrary.org/obo/GAZ_00056269">
        <obo:RO_0001025 rdf:resource="http://purl.obolibrary.org/obo/GAZ_00056254"/>
        <obo:RO_0001025 rdf:resource="http://purl.obolibrary.org/obo/GAZ_00136448"/>
        <obo:IAO_0000115>A stratovolcano that lies at the southern end of the Ruiz-Tolima massif about 20 km WNW of the city of Ibague. A 3 km wide caldera is breached to the south and contains three forested dacitic lava domes. Voluminous pyroclastic flows traveled up to 40 km from the volcano during eruptions in the mid-to-late Holocene perhaps associated with formation of the caldera. Late-Holocene eruptions produced dacitic block-and-ash flows that traveled through the breach in the caldera rim to the west and south. The latest known eruption of Volcan Cerro Machin took place about 800 years ago.</obo:IAO_0000115>
        <oboInOwl:hasOBONamespace>GAZ</oboInOwl:hasOBONamespace>
        <oboInOwl:id>GAZ:00056269</oboInOwl:id>
        <rdfs:label>Cerro Machin</rdfs:label>
    </owl:NamedIndividual>
    


    <!-- http://purl.obolibrary.org/obo/GAZ_00056270 -->

    <owl:NamedIndividual rdf:about="http://purl.obolibrary.org/obo/GAZ_00056270">
        <obo:RO_0001025 rdf:resource="http://purl.obolibrary.org/obo/GAZ_00056254"/>
        <obo:RO_0001025 rdf:resource="http://purl.obolibrary.org/obo/GAZ_00136448"/>
        <obo:IAO_0000115>A stratovolcano with a caldera open to the west. Andesitic and dacitic lava flows are of possible Holocene age. Solfataras are found on the shore of a small crater lake.</obo:IAO_0000115>
        <oboInOwl:hasOBONamespace>GAZ</oboInOwl:hasOBONamespace>
        <oboInOwl:id>GAZ:00056270</oboInOwl:id>
        <rdfs:label>Cerro Negro de Mayasquer</rdfs:label>
    </owl:NamedIndividual>
    


    <!-- http://purl.obolibrary.org/obo/GAZ_00056271 -->

    <owl:NamedIndividual rdf:about="http://purl.obolibrary.org/obo/GAZ_00056271">
        <obo:RO_0001025 rdf:resource="http://purl.obolibrary.org/obo/GAZ_00056254"/>
        <obo:RO_0001025 rdf:resource="http://purl.obolibrary.org/obo/GAZ_00136448"/>
        <obo:IAO_0000115>A stratovolcano. The southernmost historically active volcano of Colombia. The volcano is elongated in a NE-SW direction and is composed primarily of andesitic-dacitic lava flows. Two fumarolically active craters occupy the summit ridge; the main crater on the NE side and Mundo Nuevo crater on the SW side. A young lava dome occupies the 250-m-wide summit crater, and eruptions from the upper east flank produced a 6 km-long lava field. The oldest crater lies NNE of the summit crater, suggesting SW-ward migration of activity. Explosive eruptions in 1877 and 1926 are the only known historical activity from Cumbal. Fumarole fields are found in the two summit craters, and thermal springs are located on the SE flanks.</obo:IAO_0000115>
        <oboInOwl:hasOBONamespace>GAZ</oboInOwl:hasOBONamespace>
        <oboInOwl:id>GAZ:00056271</oboInOwl:id>
        <rdfs:label>Volcan Cumbal</rdfs:label>
    </owl:NamedIndividual>
    


    <!-- http://purl.obolibrary.org/obo/GAZ_00056272 -->

    <owl:NamedIndividual rdf:about="http://purl.obolibrary.org/obo/GAZ_00056272">
        <obo:RO_0001025 rdf:resource="http://purl.obolibrary.org/obo/GAZ_00056254"/>
        <obo:RO_0001025 rdf:resource="http://purl.obolibrary.org/obo/GAZ_00136448"/>
        <obo:IAO_0000115>A stratovolcano that contains two calderas, breached to the NE and SW. The summit of the andesitic-dacitic volcano is comprised of a series of post-caldera lava domes. The older caldera, open to the NE, formed during the mid-Holocene, accompanied by voluminous pyroclastic flows. The younger caldera contains the active central cone. The only historical activity of Dona Juana took place during a long-term eruption from 1897-1906, when growth of a summit lava dome was accompanied by major pyroclastic flows.</obo:IAO_0000115>
        <oboInOwl:hasOBONamespace>GAZ</oboInOwl:hasOBONamespace>
        <oboInOwl:id>GAZ:00056272</oboInOwl:id>
        <rdfs:label>Volcan Dona Juana</rdfs:label>
    </owl:NamedIndividual>
    


    <!-- http://purl.obolibrary.org/obo/GAZ_00056273 -->

    <owl:NamedIndividual rdf:about="http://purl.obolibrary.org/obo/GAZ_00056273">
        <obo:RO_0001025 rdf:resource="http://purl.obolibrary.org/obo/GAZ_00056254"/>
        <obo:RO_0001025 rdf:resource="http://purl.obolibrary.org/obo/GAZ_00136448"/>
        <obo:IAO_0000115>A stratovolcano with a large breached caldera located immediately west of the city of Pasto, is one of Colombia&apos;s most frequently active volcanoes. The dominantly andesitic Galeras volcanic complex has been active for more than 1 million years, and two major caldera collapse eruptions took place during the late Pleistocene. Long-term extensive hydrothermal alteration has affected the volcano. This has contributed to large-scale edifice collapse that has occurred on at least three occasions, producing debris avalanches that swept to the west and left a large horseshoe-shaped caldera inside which the modern cone has been constructed. Major explosive eruptions since the mid Holocene have produced widespread tephra deposits and pyroclastic flows that swept all but the southern flanks.</obo:IAO_0000115>
        <oboInOwl:hasOBONamespace>GAZ</oboInOwl:hasOBONamespace>
        <oboInOwl:id>GAZ:00056273</oboInOwl:id>
        <rdfs:label>Volcan Galeras</rdfs:label>
    </owl:NamedIndividual>
    


    <!-- http://purl.obolibrary.org/obo/GAZ_00056274 -->

    <owl:NamedIndividual rdf:about="http://purl.obolibrary.org/obo/GAZ_00056274">
        <obo:RO_0001025 rdf:resource="http://purl.obolibrary.org/obo/GAZ_00089699"/>
        <obo:RO_0001025 rdf:resource="http://purl.obolibrary.org/obo/GAZ_00136448"/>
        <obo:IAO_0000115>An elongated N-S-trending stratovolcanic chain mantled by a glacier icecap. The 5365 m high andesitic-dacitic volcano was constructed within a 10 km wide caldera. Volcanism at Nevado del Huila has produced six volcanic cones whose ages in general migrated from south to north. The high point of the complex is Pico Central. Two glacier-free lava domes lie at the southern end of the Huila volcanic complex. The first historical eruption from this little known volcano was an explosive eruption in the mid-16th century. The next eruption did not occur until 2007, when explosive activity was accompanied by damaging mudflows. Located in the Huila Department.</obo:IAO_0000115>
        <oboInOwl:hasOBONamespace>GAZ</oboInOwl:hasOBONamespace>
        <oboInOwl:id>GAZ:00056274</oboInOwl:id>
        <rdfs:label>Nevado del Huila</rdfs:label>
    </owl:NamedIndividual>
    


    <!-- http://purl.obolibrary.org/obo/GAZ_00056275 -->

    <owl:NamedIndividual rdf:about="http://purl.obolibrary.org/obo/GAZ_00056275">
        <obo:RO_0001025 rdf:resource="http://purl.obolibrary.org/obo/GAZ_00056254"/>
        <obo:RO_0001025 rdf:resource="http://purl.obolibrary.org/obo/GAZ_00089671"/>
        <obo:RO_0001025 rdf:resource="http://purl.obolibrary.org/obo/GAZ_00136448"/>
        <obo:IAO_0000115>A steep-sided, glacier-clad stratovolcano which contrasts with the broad profile of Nevado del Ruiz volcano to the north. The andesitic-dacitic younger Tolima volcano formed during the past 40,000 years, rising above and largely obscuring a 3 km wide late-Pleistocene caldera. The summit consists of a cluster of late-Pleistocene to Holocene lava domes that were associated with thick block-lava flows on the northern and eastern flanks and extensive pyroclastic-flow deposits. The summit contains a funnel-shaped crater 200-300 m deep. Holocene activity has included explosive eruptions ranging in size from moderate to plinian. The last major eruption took place about 3600 years ago. Lava dome growth has produced block-and-ash flows that traveled primarily to the NE and SE. Minor explosive eruptions have been recorded from Tolima in the 19th and 20th centuries.</obo:IAO_0000115>
        <oboInOwl:hasOBONamespace>GAZ</oboInOwl:hasOBONamespace>
        <oboInOwl:id>GAZ:00056275</oboInOwl:id>
        <rdfs:label>Nevado del Tolima</rdfs:label>
    </owl:NamedIndividual>
    


    <!-- http://purl.obolibrary.org/obo/GAZ_00056276 -->

    <owl:NamedIndividual rdf:about="http://purl.obolibrary.org/obo/GAZ_00056276">
        <rdf:type rdf:resource="http://purl.obolibrary.org/obo/ENVO_00000020"/>
        <obo:RO_0001025 rdf:resource="http://purl.obolibrary.org/obo/GAZ_00056254"/>
        <obo:RO_0001025 rdf:resource="http://purl.obolibrary.org/obo/GAZ_00089671"/>
        <obo:RO_0001025 rdf:resource="http://purl.obolibrary.org/obo/GAZ_00136448"/>
        <obo:IAO_0000115>A broad, glacier-covered volcano in central Colombia that covers &gt;200 sq km. Three major edifices, composed of andesitic and dacitic lavas and andesitic pyroclastics, have been constructed since the beginning of the Pleistocene. The modern cone consists of a broad cluster of lava domes built within the summit caldera of an older Ruiz volcano. The 1 km wide, 240-m-deep Arenas crater occupies the summit. The prominent La Olleta pyroclastic cone is located on the SW flank, and may also have been active in historical time. Steep headwalls of massive landslides cut the flanks of Nevado del Ruiz.</obo:IAO_0000115>
        <oboInOwl:hasOBONamespace>GAZ</oboInOwl:hasOBONamespace>
        <oboInOwl:id>GAZ:00056276</oboInOwl:id>
        <rdfs:label>Nevado del Ruiz</rdfs:label>
    </owl:NamedIndividual>
    


    <!-- http://purl.obolibrary.org/obo/GAZ_00056277 -->

    <owl:NamedIndividual rdf:about="http://purl.obolibrary.org/obo/GAZ_00056277">
        <obo:RO_0001025 rdf:resource="http://purl.obolibrary.org/obo/GAZ_00056254"/>
        <obo:RO_0001025 rdf:resource="http://purl.obolibrary.org/obo/GAZ_00136448"/>
        <obo:IAO_0000115>A group of stratovolcanoes.</obo:IAO_0000115>
        <oboInOwl:hasOBONamespace>GAZ</oboInOwl:hasOBONamespace>
        <oboInOwl:id>GAZ:00056277</oboInOwl:id>
        <rdfs:label>Purace Volcanic Group</rdfs:label>
    </owl:NamedIndividual>
    


    <!-- http://purl.obolibrary.org/obo/GAZ_00056278 -->

    <owl:NamedIndividual rdf:about="http://purl.obolibrary.org/obo/GAZ_00056278">
        <obo:RO_0001025 rdf:resource="http://purl.obolibrary.org/obo/GAZ_00056277"/>
        <obo:IAO_0000115>An andesitic stratovolcano with a 500-m-wide summit crater that was constructed over a dacitic shield volcano. Purace lies at the NW end of a volcanic massif opposite Pan de Azucar stratovolcano, 6 km to the SE.</obo:IAO_0000115>
        <oboInOwl:hasOBONamespace>GAZ</oboInOwl:hasOBONamespace>
        <oboInOwl:id>GAZ:00056278</oboInOwl:id>
        <rdfs:label>Volcan Purace</rdfs:label>
    </owl:NamedIndividual>
    


    <!-- http://purl.obolibrary.org/obo/GAZ_00056279 -->

    <owl:NamedIndividual rdf:about="http://purl.obolibrary.org/obo/GAZ_00056279">
        <obo:RO_0001025 rdf:resource="http://purl.obolibrary.org/obo/GAZ_00056277"/>
        <obo:IAO_0000115>A stratovolcano.</obo:IAO_0000115>
        <oboInOwl:hasOBONamespace>GAZ</oboInOwl:hasOBONamespace>
        <oboInOwl:id>GAZ:00056279</oboInOwl:id>
        <rdfs:label>Volcan Pan de Azucar</rdfs:label>
    </owl:NamedIndividual>
    


    <!-- http://purl.obolibrary.org/obo/GAZ_00056280 -->

    <owl:NamedIndividual rdf:about="http://purl.obolibrary.org/obo/GAZ_00056280">
        <obo:RO_0001025 rdf:resource="http://purl.obolibrary.org/obo/GAZ_00056277"/>
        <obo:IAO_0000115>A NW-SE-trending group of seven cones and craters that lies between the Purace and Pan de Azucar volcanoes.</obo:IAO_0000115>
        <oboInOwl:hasOBONamespace>GAZ</oboInOwl:hasOBONamespace>
        <oboInOwl:id>GAZ:00056280</oboInOwl:id>
        <rdfs:label>Los Coconucos</rdfs:label>
    </owl:NamedIndividual>
    


    <!-- http://purl.obolibrary.org/obo/GAZ_00056281 -->

    <owl:NamedIndividual rdf:about="http://purl.obolibrary.org/obo/GAZ_00056281">
        <obo:RO_0001025 rdf:resource="http://purl.obolibrary.org/obo/GAZ_00056254"/>
        <obo:RO_0001025 rdf:resource="http://purl.obolibrary.org/obo/GAZ_00136448"/>
        <obo:IAO_0000115>An andesitic-to-dacitic stratovolcano that lies at the northern end of the Ruiz-Tolima volcanic chain, NW of Cerro Bravo volcano, and lies east of the towns of Neira and Aranzazu. It has produced two young plinian pumice deposits that blanket areas NW of the volcano. The pumice deposits are separated by a soil layer radiocarbon dated at about 8460 and 7340 years ago.</obo:IAO_0000115>
        <oboInOwl:hasOBONamespace>GAZ</oboInOwl:hasOBONamespace>
        <oboInOwl:id>GAZ:00056281</oboInOwl:id>
        <rdfs:label>Volcan Caldas</rdfs:label>
    </owl:NamedIndividual>
    


    <!-- http://purl.obolibrary.org/obo/GAZ_00056282 -->

    <owl:NamedIndividual rdf:about="http://purl.obolibrary.org/obo/GAZ_00056282">
        <obo:RO_0001025 rdf:resource="http://purl.obolibrary.org/obo/GAZ_00056254"/>
        <obo:RO_0001025 rdf:resource="http://purl.obolibrary.org/obo/GAZ_00089671"/>
        <obo:RO_0001025 rdf:resource="http://purl.obolibrary.org/obo/GAZ_00136448"/>
        <obo:IAO_0000115>A small andesitic shield volcano that is dwarfed by its neighbor to the NE, Nevado del Ruiz. Holocene lava flows fill valleys SW and SE of Santa Isabel. A small Holocene lava dome was emplaced at the center of a circular depression about 10 km SW of the volcano.</obo:IAO_0000115>
        <oboInOwl:hasOBONamespace>GAZ</oboInOwl:hasOBONamespace>
        <oboInOwl:id>GAZ:00056282</oboInOwl:id>
        <rdfs:label>Volcan Santa Isabel</rdfs:label>
    </owl:NamedIndividual>
    


    <!-- http://purl.obolibrary.org/obo/GAZ_00056283 -->

    <owl:NamedIndividual rdf:about="http://purl.obolibrary.org/obo/GAZ_00056283">
        <obo:RO_0001025 rdf:resource="http://purl.obolibrary.org/obo/GAZ_00056254"/>
        <obo:RO_0001025 rdf:resource="http://purl.obolibrary.org/obo/GAZ_00136448"/>
        <obo:IAO_0000115>An andesitic-dacitic stratovolcano located about 25 km SSE of Popayan city in southern Colombia, SW of Purace volcano. Three calderas, 4.5, 2.5, and 1 km in diameter, are found on Sotara, giving the summit an irregular profile. No historical eruptions are known from Sotara, however the volcano currently displays fumarolic and hot spring activity.</obo:IAO_0000115>
        <oboInOwl:hasOBONamespace>GAZ</oboInOwl:hasOBONamespace>
        <oboInOwl:id>GAZ:00056283</oboInOwl:id>
        <rdfs:label>Volcan Sotara</rdfs:label>
    </owl:NamedIndividual>
    


    <!-- http://purl.obolibrary.org/obo/GAZ_00056284 -->

    <owl:NamedIndividual rdf:about="http://purl.obolibrary.org/obo/GAZ_00056284">
        <obo:RO_0001025 rdf:resource="http://purl.obolibrary.org/obo/GAZ_00056254"/>
        <obo:RO_0001025 rdf:resource="http://purl.obolibrary.org/obo/GAZ_00136448"/>
        <obo:IAO_0000115>A lava dome near the boundary of Narino and Cauca provinces in southern Colombia NE of Dona Juana volcano. Many morphologically fresh cones are located nearby (Von Wolff, 1929), although the age of the most recent eruption is not known.</obo:IAO_0000115>
        <oboInOwl:hasOBONamespace>GAZ</oboInOwl:hasOBONamespace>
        <oboInOwl:id>GAZ:00056284</oboInOwl:id>
        <rdfs:label>Volcan Petacas</rdfs:label>
    </owl:NamedIndividual>
    


    <!-- http://purl.obolibrary.org/obo/GAZ_00056286 -->

    <owl:NamedIndividual rdf:about="http://purl.obolibrary.org/obo/GAZ_00056286">
        <obo:RO_0001025 rdf:resource="http://purl.obolibrary.org/obo/GAZ_00136448"/>
        <obo:IAO_0000115>An extinct volcano on the western side of Sangay National Park in Ecuador, 170 km south of Quito.</obo:IAO_0000115>
        <oboInOwl:hasOBONamespace>GAZ</oboInOwl:hasOBONamespace>
        <oboInOwl:id>GAZ:00056286</oboInOwl:id>
        <rdfs:label>Volcan El Altar Volcano</rdfs:label>
    </owl:NamedIndividual>
    


    <!-- http://purl.obolibrary.org/obo/GAZ_00056287 -->

    <owl:NamedIndividual rdf:about="http://purl.obolibrary.org/obo/GAZ_00056287">
        <obo:RO_0001025 rdf:resource="http://purl.obolibrary.org/obo/GAZ_00056289"/>
        <obo:RO_0001025 rdf:resource="http://purl.obolibrary.org/obo/GAZ_00136448"/>
        <obo:IAO_0000115>A steep-sided andesitic-dacitic stratovolcano that towers more than 3 km above its northern base, is one of Ecuador&apos;s most active volcanoes. Three major volcanic edifices have been sequentially constructed since the mid-Pleistocene over a basement of metamorphic rocks. Tungurahua II was built within the past 14,000 years following the collapse of the initial edifice. Tungurahua II itself collapsed about 3000 years ago and produced a large debris-avalanche deposit and a horseshoe-shaped caldera open to the west, inside which the modern glacier-capped stratovolcano (Tungurahua III) was constructed. Historical eruptions have all originated from the summit crater. They have been accompanied by strong explosions and sometimes by pyroclastic flows and lava flows that reached populated areas at the volcano&apos;s base. Prior to a long-term eruption beginning in 1999 that caused the temporary evacuation of the city of Banos at the foot of the volcano, the last major eruption had occurred from 1916 to 1918, although minor activity continued until 1925.</obo:IAO_0000115>
        <oboInOwl:hasOBONamespace>GAZ</oboInOwl:hasOBONamespace>
        <oboInOwl:id>GAZ:00056287</oboInOwl:id>
        <rdfs:label>Volcan Tungurahua</rdfs:label>
    </owl:NamedIndividual>
    


    <!-- http://purl.obolibrary.org/obo/GAZ_00056288 -->

    <owl:NamedIndividual rdf:about="http://purl.obolibrary.org/obo/GAZ_00056288">
        <oboInOwl:hasOBONamespace>GAZ</oboInOwl:hasOBONamespace>
        <oboInOwl:id>GAZ:00056288</oboInOwl:id>
        <rdfs:label>Cordillera Central</rdfs:label>
    </owl:NamedIndividual>
    


    <!-- http://purl.obolibrary.org/obo/GAZ_00056289 -->

    <owl:NamedIndividual rdf:about="http://purl.obolibrary.org/obo/GAZ_00056289">
        <obo:RO_0001025 rdf:resource="http://purl.obolibrary.org/obo/GAZ_00056288"/>
        <obo:IAO_0000115>A chain of mountains in the Andes of Ecuador, the chief of them volcanic. They are continued in the Cordillera Central of Peru in the South and Cordillera Central of Colombia in the North. The Cordillera Real includes the Antisana, Cotopaxi, and Cayambe, while Chimborazo is in the Cordillera Occidental.</obo:IAO_0000115>
        <oboInOwl:hasOBONamespace>GAZ</oboInOwl:hasOBONamespace>
        <oboInOwl:id>GAZ:00056289</oboInOwl:id>
        <rdfs:label>Cordillera Central of Ecuador</rdfs:label>
    </owl:NamedIndividual>
    


    <!-- http://purl.obolibrary.org/obo/GAZ_00056290 -->

    <owl:NamedIndividual rdf:about="http://purl.obolibrary.org/obo/GAZ_00056290">
        <obo:RO_0001025 rdf:resource="http://purl.obolibrary.org/obo/GAZ_00056289"/>
        <obo:RO_0001025 rdf:resource="http://purl.obolibrary.org/obo/GAZ_00136448"/>
        <obo:IAO_0000115>An isolated stratovolcano, located east of the Andean crest. It is the southernmost of Ecuador&apos;s volcanoes, and its most active. The dominantly andesitic volcano has been in frequent eruption for the past several centuries. The steep-sided, 5230 m high glacier-covered volcano grew within horseshoe-shaped calderas of two previous edifices, which were destroyed by collapse to the east, producing large debris avalanches that reached the Amazonian lowlands. The modern edifice dates back to at least 14,000 years ago. Sangay towers above the tropical jungle on the east side; on the other sides flat plains of ash from the volcano have been sculpted by heavy rains into steep-walled canyons up to 600 m deep. The earliest report of a historical eruption was in 1628. More or less continuous eruptions were reported from 1728 until 1916, and again from 1934 to the present. The more or less constant eruptive activity has caused frequent changes to the morphology of the summit crater complex.</obo:IAO_0000115>
        <oboInOwl:hasOBONamespace>GAZ</oboInOwl:hasOBONamespace>
        <oboInOwl:id>GAZ:00056290</oboInOwl:id>
        <rdfs:label>Volcan Sangay Volcano</rdfs:label>
    </owl:NamedIndividual>
    


    <!-- http://purl.obolibrary.org/obo/GAZ_00056292 -->

    <owl:NamedIndividual rdf:about="http://purl.obolibrary.org/obo/GAZ_00056292">
        <obo:RO_0001025 rdf:resource="http://purl.obolibrary.org/obo/GAZ_00056289"/>
        <obo:RO_0001025 rdf:resource="http://purl.obolibrary.org/obo/GAZ_00136448"/>
        <obo:IAO_0000115>A massive, glacier-covered stratovolcano NE of Cotopaxi, along the western margin of the Cordillera Real, 50 km SE of Quito. An older edifice forming the east side of the volcano was constructed over granitic and metasedimentary rocks and is itself overtopped on its NW side by the modern edifice. Two small calderas, one breached to the south and the other to the NE, truncate the older edifice. Viscous, youthful block lava flows have issued from radial fissures on the flanks of 5753 m high Antisana, one of the highest peaks in Ecuador.</obo:IAO_0000115>
        <oboInOwl:hasOBONamespace>GAZ</oboInOwl:hasOBONamespace>
        <oboInOwl:id>GAZ:00056292</oboInOwl:id>
        <rdfs:label>Volcan Antisana</rdfs:label>
    </owl:NamedIndividual>
    


    <!-- http://purl.obolibrary.org/obo/GAZ_00056293 -->

    <owl:NamedIndividual rdf:about="http://purl.obolibrary.org/obo/GAZ_00056293">
        <obo:RO_0001025 rdf:resource="http://purl.obolibrary.org/obo/GAZ_00056252"/>
        <obo:RO_0001025 rdf:resource="http://purl.obolibrary.org/obo/GAZ_00136448"/>
        <obo:IAO_0000115>A volcanic caldera neighboured by Ecuador&apos;s highest mountain Chimborazo. Carihuairazo is located in the Cordillera Occidental of the Andes of central Ecuador, 150 km south-southwest of the capital Quito. Its neighboured by 6,267 m high Chimborazo. The nearest cities are Riobamba (~30 km to the southeast), Ambato (~30 km to the northeast) and Guaranda (~30 km to the southwest). Carihuairazo&apos;s 1.5 km wide heavy eroded caldera opens to the east.</obo:IAO_0000115>
        <oboInOwl:hasOBONamespace>GAZ</oboInOwl:hasOBONamespace>
        <oboInOwl:id>GAZ:00056293</oboInOwl:id>
        <rdfs:label>Carihuairazo Caldera</rdfs:label>
    </owl:NamedIndividual>
    


    <!-- http://purl.obolibrary.org/obo/GAZ_00056294 -->

    <owl:NamedIndividual rdf:about="http://purl.obolibrary.org/obo/GAZ_00056294">
        <obo:RO_0001025 rdf:resource="http://purl.obolibrary.org/obo/GAZ_00056263"/>
        <oboInOwl:hasOBONamespace>GAZ</oboInOwl:hasOBONamespace>
        <oboInOwl:id>GAZ:00056294</oboInOwl:id>
        <rdfs:label>Cordillera Oriental of Ecuador</rdfs:label>
    </owl:NamedIndividual>
    


    <!-- http://purl.obolibrary.org/obo/GAZ_00056295 -->

    <owl:NamedIndividual rdf:about="http://purl.obolibrary.org/obo/GAZ_00056295">
        <obo:RO_0001025 rdf:resource="http://purl.obolibrary.org/obo/GAZ_00056289"/>
        <obo:RO_0001025 rdf:resource="http://purl.obolibrary.org/obo/GAZ_00136448"/>
        <obo:IAO_0000115>A massive compound andesitic-dacitic stratovolcano that is located on the isolated western edge of the Cordillera Real, east of the Inter-Andean Valley. The 5790 m high volcano, whose southern flank lies astride the equator, is capped by extensive glaciers, which descend to 4200 m on the eastern Amazonian side. The modern Nevado Cayambe volcano, constructed to the east of older Pleistocene volcanic complexes, contains two summit lava domes located about 1.5 km apart, the western of which is the highest. Several other lava domes on the upper flanks have been the source of pyroclastic flows that reached the lower flanks of the volcano. A prominent Holocene pyroclastic cone on the lower eastern flank, La Virgen, fed thick andesitic lava flows that traveled about 10 km to the east. Nevado Cayambe was recently discovered to have produced frequent explosive eruptions during the Holocene beginning about 4000 years ago, and to have had a single historical eruption, during 1785-86.</obo:IAO_0000115>
        <oboInOwl:hasOBONamespace>GAZ</oboInOwl:hasOBONamespace>
        <oboInOwl:id>GAZ:00056295</oboInOwl:id>
        <rdfs:label>Volcan Cayambe</rdfs:label>
    </owl:NamedIndividual>
    


    <!-- http://purl.obolibrary.org/obo/GAZ_00056296 -->

    <owl:NamedIndividual rdf:about="http://purl.obolibrary.org/obo/GAZ_00056296">
        <obo:RO_0001025 rdf:resource="http://purl.obolibrary.org/obo/GAZ_00056252"/>
        <obo:RO_0001025 rdf:resource="http://purl.obolibrary.org/obo/GAZ_00136448"/>
        <obo:IAO_0000115>A dominantly andesitic-to-dacitic stratovolcano that is mostly of Pliocene-to-Pleistocene age. The volcano collapsed about 35,000 years ago, producing a major debris avalanche, whose deposits underlie Riobamba and temporarily dammed the Rio Chambo, producing an ephemeral lake. Subsequent eruptions have been dominantly andesitic and constructed three edifices along an east-west line, the youngest and westernmost of which forms the current summit of Chimborazo. Although activity was once thought to have ceased during the very latest Pleistocene, recent work indicates that Chimborazo erupted several times during the Holocene, producing pyroclastic surges that reached down to 3800 m elevation.</obo:IAO_0000115>
        <oboInOwl:hasOBONamespace>GAZ</oboInOwl:hasOBONamespace>
        <oboInOwl:id>GAZ:00056296</oboInOwl:id>
        <rdfs:label>Volcan Chimborazo</rdfs:label>
    </owl:NamedIndividual>
    


    <!-- http://purl.obolibrary.org/obo/GAZ_00056297 -->

    <owl:NamedIndividual rdf:about="http://purl.obolibrary.org/obo/GAZ_00056297">
        <obo:RO_0001025 rdf:resource="http://purl.obolibrary.org/obo/GAZ_00136448"/>
        <obo:IAO_0000115>A dormant, eroded volcano of Ecuador. It is situated about 30 km southwest of Quito in the western slopes of the Andes.</obo:IAO_0000115>
        <oboInOwl:hasOBONamespace>GAZ</oboInOwl:hasOBONamespace>
        <oboInOwl:id>GAZ:00056297</oboInOwl:id>
        <rdfs:label>Volcan Corazon</rdfs:label>
    </owl:NamedIndividual>
    


    <!-- http://purl.obolibrary.org/obo/GAZ_00056298 -->

    <owl:NamedIndividual rdf:about="http://purl.obolibrary.org/obo/GAZ_00056298">
        <obo:RO_0001025 rdf:resource="http://purl.obolibrary.org/obo/GAZ_00056289"/>
        <obo:RO_0001025 rdf:resource="http://purl.obolibrary.org/obo/GAZ_00136448"/>
        <obo:IAO_0000115>A glacier-clad stratovolcano. The steep-sided cone is capped by nested summit craters, the largest of which is about 550 x 800 m in diameter. Deep valleys scoured by lahars radiate from the summit of the andesitic volcano, and large andesitic lava flows extend as far as the base of Cotopaxi. The modern conical volcano has been constructed since a major edifice collapse sometime prior to about 5000 years ago. Pyroclastic flows (often confused in historical accounts with lava flows) have accompanied many explosive eruptions of Cotopaxi, and lahars have frequently devastated adjacent valleys. The most violent historical eruptions took place in 1744, 1768, and 1877. Pyroclastic flows descended all sides of the volcano in 1877, and lahars traveled more than 100 km into the Pacific Ocean and western Amazon basin. The last significant eruption of Cotopaxi took place in 1904.</obo:IAO_0000115>
        <oboInOwl:hasOBONamespace>GAZ</oboInOwl:hasOBONamespace>
        <oboInOwl:id>GAZ:00056298</oboInOwl:id>
        <rdfs:label>Volcan Cotopaxi</rdfs:label>
    </owl:NamedIndividual>
    


    <!-- http://purl.obolibrary.org/obo/GAZ_00056299 -->

    <owl:NamedIndividual rdf:about="http://purl.obolibrary.org/obo/GAZ_00056299">
        <obo:RO_0001025 rdf:resource="http://purl.obolibrary.org/obo/GAZ_00056252"/>
        <obo:RO_0001025 rdf:resource="http://purl.obolibrary.org/obo/GAZ_00136448"/>
        <obo:IAO_0000115>A caldera located at the southern foot of the sharp-peaked Pleistocene Cotacachi stratovolcano about 100 km north of Quito. The 3 km wide caldera was created during a major explosive eruption about 3100 years ago that produced nearly 5 cu km of pyroclastic-flow and -fall deposits. Cuicocha contains four intra-caldera dacitic lava domes that form two steep-sided forested islands in the large lake. A pre-caldera Cuicocha lava dome is situated on the east side of the lake. Pyroclastic-flow deposits cover wide areas around the low-rimmed caldera.</obo:IAO_0000115>
        <oboInOwl:hasOBONamespace>GAZ</oboInOwl:hasOBONamespace>
        <oboInOwl:id>GAZ:00056299</oboInOwl:id>
        <rdfs:label>Cuicocha Caldera</rdfs:label>
    </owl:NamedIndividual>
    


    <!-- http://purl.obolibrary.org/obo/GAZ_00056300 -->

    <owl:NamedIndividual rdf:about="http://purl.obolibrary.org/obo/GAZ_00056300">
        <obo:RO_0001025 rdf:resource="http://purl.obolibrary.org/obo/GAZ_00056299"/>
        <obo:IAO_0000115>A caldera lake at the foot of Cotacachi Volcano in the Cordillera Occidental of the Ecuadorian Andes.</obo:IAO_0000115>
        <oboInOwl:hasOBONamespace>GAZ</oboInOwl:hasOBONamespace>
        <oboInOwl:id>GAZ:00056300</oboInOwl:id>
        <rdfs:label>Laguna Cuicoch</rdfs:label>
    </owl:NamedIndividual>
    


    <!-- http://purl.obolibrary.org/obo/GAZ_00056301 -->

    <owl:NamedIndividual rdf:about="http://purl.obolibrary.org/obo/GAZ_00056301">
        <obo:RO_0001025 rdf:resource="http://purl.obolibrary.org/obo/GAZ_00136448"/>
        <obo:IAO_0000115>A compount volcano that rises to the north above scenic Laguna de San Pablo in the Interandean valley about 60 km north of Quito. The main edifice, Taita Imbabura (&quot;Father Imbabura&quot;) forms the summit, with Huarmi Imbabura (&quot;Imbabura&apos;s Son&quot;) forming a lateral lava-dome complex on the SW flank. Activity at the Pleistocene Imbabura I edifice constructed a large andesitic stratovolcano and ended prior to about 43,000 years ago with a major collapse that produced a debris avalanche that traveled 16 km to the north. Subsequent growth of the Imbabura II stratovolcano continued at least into the early Holocene and typically consisted of growth and collapse of large-volume dacitic lava domes. A major eruption about 25,000 years ago produced a debris avalanche and possible lateral blast and was followed by growth of the Huarmi Imbabura lava dome. Historical reports of eruptions consisted of only mudflows and rock slides.</obo:IAO_0000115>
        <oboInOwl:hasOBONamespace>GAZ</oboInOwl:hasOBONamespace>
        <oboInOwl:id>GAZ:00056301</oboInOwl:id>
        <rdfs:label>Volcan Imbabura</rdfs:label>
    </owl:NamedIndividual>
    


    <!-- http://purl.obolibrary.org/obo/GAZ_00056302 -->

    <owl:NamedIndividual rdf:about="http://purl.obolibrary.org/obo/GAZ_00056302">
        <obo:RO_0001025 rdf:resource="http://purl.obolibrary.org/obo/GAZ_00136448"/>
        <obo:IAO_0000115>A dormant stratovolcano with two major peaks. Iliniza Norte lies 1.8 km NNW of the higher peak, 5248-m Iliniza Sur. The dominantly andesitic-to-dacitic Iliniza is largely, if not entirely Pleistocene in age. However, the Tishigcuchi (Rasuyacu) lava dome on the south flank was active during the Holocene. Recent work suggests that Iliniza itself, which is substantially eroded, may have had relatively young eruptions. Iliniza Norte is a remnant of the main volcanic edifice, and the younger Iliniza Sur is an andesitic-dacitic stratovolcano surrounded by thick pyroclastic-flow deposits. An explosive eruption formed a small caldera, which is partially filled by a lava dome forming the summit of Iliniza Sur. Two lava domes are found on the southern and NE flanks of the complex.</obo:IAO_0000115>
        <oboInOwl:hasOBONamespace>GAZ</oboInOwl:hasOBONamespace>
        <oboInOwl:id>GAZ:00056302</oboInOwl:id>
        <rdfs:label>Volcan Illiniza</rdfs:label>
    </owl:NamedIndividual>
    


    <!-- http://purl.obolibrary.org/obo/GAZ_00056303 -->

    <owl:NamedIndividual rdf:about="http://purl.obolibrary.org/obo/GAZ_00056303">
        <obo:RO_0001025 rdf:resource="http://purl.obolibrary.org/obo/GAZ_00056300"/>
        <obo:IAO_0000115>An island formed from two dacitic lava domes.</obo:IAO_0000115>
        <oboInOwl:hasOBONamespace>GAZ</oboInOwl:hasOBONamespace>
        <oboInOwl:id>GAZ:00056303</oboInOwl:id>
        <rdfs:label>Yerovi Island</rdfs:label>
    </owl:NamedIndividual>
    


    <!-- http://purl.obolibrary.org/obo/GAZ_00056304 -->

    <owl:NamedIndividual rdf:about="http://purl.obolibrary.org/obo/GAZ_00056304">
        <obo:RO_0001025 rdf:resource="http://purl.obolibrary.org/obo/GAZ_00056300"/>
        <obo:IAO_0000115>An island formed from two dacitic lava domes.</obo:IAO_0000115>
        <oboInOwl:hasOBONamespace>GAZ</oboInOwl:hasOBONamespace>
        <oboInOwl:id>GAZ:00056304</oboInOwl:id>
        <rdfs:label>Teodoro Wolf Island</rdfs:label>
    </owl:NamedIndividual>
    


    <!-- http://purl.obolibrary.org/obo/GAZ_00056306 -->

    <owl:NamedIndividual rdf:about="http://purl.obolibrary.org/obo/GAZ_00056306">
        <obo:RO_0001025 rdf:resource="http://purl.obolibrary.org/obo/GAZ_00136448"/>
        <obo:IAO_0000115>A volcano.</obo:IAO_0000115>
        <oboInOwl:hasOBONamespace>GAZ</oboInOwl:hasOBONamespace>
        <oboInOwl:id>GAZ:00056306</oboInOwl:id>
        <rdfs:label>Volcan Cotacachi</rdfs:label>
    </owl:NamedIndividual>
    


    <!-- http://purl.obolibrary.org/obo/GAZ_00056307 -->

    <owl:NamedIndividual rdf:about="http://purl.obolibrary.org/obo/GAZ_00056307">
        <obo:RO_0001025 rdf:resource="http://purl.obolibrary.org/obo/GAZ_00056302"/>
        <obo:IAO_0000115>A peak of the Illiniza Volcano.</obo:IAO_0000115>
        <oboInOwl:hasOBONamespace>GAZ</oboInOwl:hasOBONamespace>
        <oboInOwl:id>GAZ:00056307</oboInOwl:id>
        <rdfs:label>Illiniza Norte</rdfs:label>
    </owl:NamedIndividual>
    


    <!-- http://purl.obolibrary.org/obo/GAZ_00056308 -->

    <owl:NamedIndividual rdf:about="http://purl.obolibrary.org/obo/GAZ_00056308">
        <obo:RO_0001025 rdf:resource="http://purl.obolibrary.org/obo/GAZ_00056302"/>
        <obo:IAO_0000115>A peak of the Illiniza Volcano.</obo:IAO_0000115>
        <oboInOwl:hasOBONamespace>GAZ</oboInOwl:hasOBONamespace>
        <oboInOwl:id>GAZ:00056308</oboInOwl:id>
        <rdfs:label>Illiniza Sud</rdfs:label>
    </owl:NamedIndividual>
    


    <!-- http://purl.obolibrary.org/obo/GAZ_00056309 -->

    <owl:NamedIndividual rdf:about="http://purl.obolibrary.org/obo/GAZ_00056309">
        <obo:RO_0001025 rdf:resource="http://purl.obolibrary.org/obo/GAZ_00056294"/>
        <obo:RO_0001025 rdf:resource="http://purl.obolibrary.org/obo/GAZ_00136448"/>
        <obo:IAO_0000115>A complex of stratovolcanoes. An earlier Mojanda edifice contains remnants of a larger earlier caldera and a smaller summit caldera occupied by two lakes. The andesitic-to-rhyolitic Fuya Fuya volcano was constructed contemporaneously immediately to the west of Mojanda and produced two major rhyolitic plinian explosive eruptions, possibly associated with caldera formation. Fuya Fuya underwent edifice collapse less than 165,000 years ago, leaving a large horseshoe-shaped caldera open to the west. Subsequently, a new composite cone and dacitic lava domes were extruded inside the caldera. The youngest domes were possibly extruded during the latest Pleistocene, and Holocene eruptive activity is uncertain.</obo:IAO_0000115>
        <oboInOwl:hasOBONamespace>GAZ</oboInOwl:hasOBONamespace>
        <oboInOwl:id>GAZ:00056309</oboInOwl:id>
        <rdfs:label>Volcan Mojanda</rdfs:label>
    </owl:NamedIndividual>
    


    <!-- http://purl.obolibrary.org/obo/GAZ_00056310 -->

    <owl:NamedIndividual rdf:about="http://purl.obolibrary.org/obo/GAZ_00056310">
        <obo:RO_0001025 rdf:resource="http://purl.obolibrary.org/obo/GAZ_00136448"/>
        <obo:IAO_0000115>A volcano located in the Guayllabamba river basin in the Ecuadorean Andes.</obo:IAO_0000115>
        <oboInOwl:hasOBONamespace>GAZ</oboInOwl:hasOBONamespace>
        <oboInOwl:id>GAZ:00056310</oboInOwl:id>
        <rdfs:label>Volcan Pasochoa</rdfs:label>
    </owl:NamedIndividual>
    


    <!-- http://purl.obolibrary.org/obo/GAZ_00056311 -->

    <owl:NamedIndividual rdf:about="http://purl.obolibrary.org/obo/GAZ_00056311">
        <obo:RO_0001025 rdf:resource="http://purl.obolibrary.org/obo/GAZ_00136448"/>
        <obo:IAO_0000115>A stratovolcano. With Ruca Pichincha, forms a broad volcanic massif that rises immediately to the west of Ecuador&apos;s capital city, Quito. A lava dome is located at the head of a 6 km wide breached caldera that formed during a late-Pleistocene slope failure of Guagua Pichincha about 50,000 years ago. Subsequent late-Pleistocene and Holocene eruptions from the central vent in the breached caldera consisted of explosive activity with pyroclastic flows accompanied by periodic growth and destruction of the central lava dome. Many minor eruptions have occurred since the beginning of the Spanish era at Guagua Pichincha, which is one of Ecuador&apos;s most active volcanoes. The largest historical eruption took place in 1660, when ash fell over a 1000 km radius, accumulating to 30 cm depth in Quito. Pyroclastic flows and surges also occurred, primarily to the west, and affected agricultural activity, causing great economic losses.</obo:IAO_0000115>
        <oboInOwl:hasOBONamespace>GAZ</oboInOwl:hasOBONamespace>
        <oboInOwl:id>GAZ:00056311</oboInOwl:id>
        <rdfs:label>Volcan Pichincha</rdfs:label>
    </owl:NamedIndividual>
    


    <!-- http://purl.obolibrary.org/obo/GAZ_00056313 -->

    <owl:NamedIndividual rdf:about="http://purl.obolibrary.org/obo/GAZ_00056313">
        <obo:RO_0001025 rdf:resource="http://purl.obolibrary.org/obo/GAZ_00056252"/>
        <obo:RO_0001025 rdf:resource="http://purl.obolibrary.org/obo/GAZ_00136448"/>
        <obo:IAO_0000115>A truncated, forested dacitic cone that is the westernmost of Ecuador&apos;s Andean volcanoes. It is located at the margin of the Western Cordillera 35 km WNW of the city of Latacunga and contains a 3 km wide caldera with steep-sided walls that rise 400 m above the surface of 250-m-deep caldera lake. Lava domes form the caldera&apos;s perimeter and occupy its floor. This small volcano has produced major explosive eruptions every 10-14,000 years during the past 40,000 years. Its most recent large eruption about 800 radiocarbon years ago produced voluminous pyroclastic flows, lahars that reached the Pacific Ocean, and one of the largest airfall-tephra deposits of the northern Andes. Formation of the caldera was followed by extrusion of a small lava dome. Reports of historical eruptions from the caldera lake are somewhat ambiguous. Fumaroles are present on the lake floor and hot springs occur on the eastern flank.</obo:IAO_0000115>
        <oboInOwl:hasOBONamespace>GAZ</oboInOwl:hasOBONamespace>
        <oboInOwl:id>GAZ:00056313</oboInOwl:id>
        <rdfs:label>Quilotoa Caldera</rdfs:label>
    </owl:NamedIndividual>
    


    <!-- http://purl.obolibrary.org/obo/GAZ_00056314 -->

    <owl:NamedIndividual rdf:about="http://purl.obolibrary.org/obo/GAZ_00056314">
        <obo:RO_0001025 rdf:resource="http://purl.obolibrary.org/obo/GAZ_00056289"/>
        <obo:RO_0001025 rdf:resource="http://purl.obolibrary.org/obo/GAZ_00136448"/>
        <obo:IAO_0000115>The most frequently active of a chain of Ecuadorian volcanoes in the Cordillera Real, well east of the principal volcanic axis. The forested, dominantly andesitic Volcan El Reventador stratovolcano rises to 3562 m above the jungles of the western Amazon basin. A 4 km wide caldera widely breached to the east was formed by edifice collapse and is partially filled by a young, unvegetated stratovolcano that rises about 1300 m above the caldera floor to a height comparable to the caldera rim. Reventador has been the source of numerous lava flows as well as explosive eruptions that were visible from Quito in historical time. Frequent lahars in this region of heavy rainfall have constructed a debris plain on the eastern floor of the caldera. The largest historical eruption at Reventador took place in 2002, producing a 17 km-high eruption column, pyroclastic flows that traveled up to 8 km, and lava flows from summit and flank vents.</obo:IAO_0000115>
        <oboInOwl:hasOBONamespace>GAZ</oboInOwl:hasOBONamespace>
        <oboInOwl:id>GAZ:00056314</oboInOwl:id>
        <rdfs:label>Volcan Reventador Volcano</rdfs:label>
    </owl:NamedIndividual>
    


    <!-- http://purl.obolibrary.org/obo/GAZ_00056315 -->

    <owl:NamedIndividual rdf:about="http://purl.obolibrary.org/obo/GAZ_00056315">
        <obo:RO_0001025 rdf:resource="http://purl.obolibrary.org/obo/GAZ_00136448"/>
        <obo:IAO_0000115>A dormant, heavily-eroded volcano 4721 m above sea level. Situated in the Andes mountains 40 km south of Quito, Ecuador.</obo:IAO_0000115>
        <oboInOwl:hasOBONamespace>GAZ</oboInOwl:hasOBONamespace>
        <oboInOwl:id>GAZ:00056315</oboInOwl:id>
        <rdfs:label>Volcan Ruminahui</rdfs:label>
    </owl:NamedIndividual>
    


    <!-- http://purl.obolibrary.org/obo/GAZ_00056316 -->

    <owl:NamedIndividual rdf:about="http://purl.obolibrary.org/obo/GAZ_00056316">
        <obo:RO_0001025 rdf:resource="http://purl.obolibrary.org/obo/GAZ_00136448"/>
        <obo:IAO_0000115>A small stratovolcano near the Colombia border, is the northernmost of a chain of Ecuadorian volcanoes east of the principal volcanic axis. The dominantly dacitic Soche volcano was constructed over Paleozoic rocks and has a summit caldera that opens towards the east. A major explosive eruption took place during the early Holocene. The ejection of voluminous dacitic airfall pumice and pyroclastic flows was followed by the formation of two lava domes in the caldera.</obo:IAO_0000115>
        <oboInOwl:hasOBONamespace>GAZ</oboInOwl:hasOBONamespace>
        <oboInOwl:id>GAZ:00056316</oboInOwl:id>
        <rdfs:label>Volcan el Soche</rdfs:label>
    </owl:NamedIndividual>
    


    <!-- http://purl.obolibrary.org/obo/GAZ_00056317 -->

    <owl:NamedIndividual rdf:about="http://purl.obolibrary.org/obo/GAZ_00056317">
        <obo:RO_0001025 rdf:resource="http://purl.obolibrary.org/obo/GAZ_00056309"/>
        <obo:IAO_0000115>A stratovolcano.</obo:IAO_0000115>
        <oboInOwl:hasOBONamespace>GAZ</oboInOwl:hasOBONamespace>
        <oboInOwl:id>GAZ:00056317</oboInOwl:id>
        <rdfs:label>Cushinirumi Volcano</rdfs:label>
    </owl:NamedIndividual>
    


    <!-- http://purl.obolibrary.org/obo/GAZ_00056318 -->

    <owl:NamedIndividual rdf:about="http://purl.obolibrary.org/obo/GAZ_00056318">
        <obo:RO_0001025 rdf:resource="http://purl.obolibrary.org/obo/GAZ_00056309"/>
        <obo:IAO_0000115>A stratovolcano.</obo:IAO_0000115>
        <oboInOwl:hasOBONamespace>GAZ</oboInOwl:hasOBONamespace>
        <oboInOwl:id>GAZ:00056318</oboInOwl:id>
        <rdfs:label>Fuya Fuya Volcano</rdfs:label>
    </owl:NamedIndividual>
    


    <!-- http://purl.obolibrary.org/obo/GAZ_00056319 -->

    <owl:NamedIndividual rdf:about="http://purl.obolibrary.org/obo/GAZ_00056319">
        <obo:RO_0001025 rdf:resource="http://purl.obolibrary.org/obo/GAZ_00056309"/>
        <obo:IAO_0000115>A stratovolcano.</obo:IAO_0000115>
        <oboInOwl:hasOBONamespace>GAZ</oboInOwl:hasOBONamespace>
        <oboInOwl:id>GAZ:00056319</oboInOwl:id>
        <rdfs:label>San Bartolo Volcano</rdfs:label>
    </owl:NamedIndividual>
    


    <!-- http://purl.obolibrary.org/obo/GAZ_00056322 -->

    <owl:NamedIndividual rdf:about="http://purl.obolibrary.org/obo/GAZ_00056322">
        <obo:RO_0001025 rdf:resource="http://purl.obolibrary.org/obo/GAZ_00136448"/>
        <obo:IAO_0000115>A stratovolcano, located about 25 km SW of the capital city of Quito. It consists of a large Pleistocene andesitic stratovolcanoes truncated by a late-Pleistocene to Holocene caldera. Growth of Carcacha stratovolcano was followed by construction of Atacazo, a stratovolcano with flank lava domes. The 6 km wide caldera, which is breached to the SW, is partially filled by three dacitic lava-dome complexes of Holocene age. Two andesitic lava domes are also found on the SE flank. Several plinian eruptions have occurred at the Atacazo-Ninahuilca complex during the Holocene, accompanied by growth of lava domes. The latest dated eruption took place about 2300 years ago, forming the Ninahuilca lava domes within the summit caldera. Dome formation was accompanied by plinian explosive eruptions and pyroclastic flows that traveled 35 km down valleys to the west.</obo:IAO_0000115>
        <oboInOwl:hasOBONamespace>GAZ</oboInOwl:hasOBONamespace>
        <oboInOwl:id>GAZ:00056322</oboInOwl:id>
        <rdfs:label>Volcan Atacazo</rdfs:label>
    </owl:NamedIndividual>
    


    <!-- http://purl.obolibrary.org/obo/GAZ_00056323 -->

    <owl:NamedIndividual rdf:about="http://purl.obolibrary.org/obo/GAZ_00056323">
        <obo:RO_0001025 rdf:resource="http://purl.obolibrary.org/obo/GAZ_00136448"/>
        <obo:IAO_0000115>A massive, eroded caldera complex of Pliocene-Holocene age that forms one of the largest rhyolitic centers of the northern Andes. The caldera is 32 km long in the N-S direction and 18-24 km wide in the E-W direction. Chacana was constructed during three cycles of andesitic-to-rhyolitic volcanism. Dacitic lava flows were erupted from caldera-floor fissures between 30,000 and 21,000 years ago. Numerous lava domes were constructed within the caldera, which has been the source of frequent explosive eruptions throughout the Holocene as well as historical lava flows during the 18th century. The massive Antisana stratovolcano was constructed immediately to the SE.</obo:IAO_0000115>
        <oboInOwl:hasOBONamespace>GAZ</oboInOwl:hasOBONamespace>
        <oboInOwl:id>GAZ:00056323</oboInOwl:id>
        <rdfs:label>Chacana Caldera</rdfs:label>
    </owl:NamedIndividual>
    


    <!-- http://purl.obolibrary.org/obo/GAZ_00056324 -->

    <owl:NamedIndividual rdf:about="http://purl.obolibrary.org/obo/GAZ_00056324">
        <obo:RO_0001025 rdf:resource="http://purl.obolibrary.org/obo/GAZ_00136448"/>
        <obo:IAO_0000115>A stratovolcano that rises 2800 m above the jungles of the western Amazon basin, east of Antisana volcano, and occupies an isolated position far to the east of the main Andes volcanic axis. Constructed over Cretaceous sedimentary rocks, 3990 m high Sumaco forms a relatively symmetrical cone in an area of heavy rainfall and erosion. Sumaco has produced alkaline tephritic, basanitic, and phonolitic rocks distinct from those of the main Andean chain. The volcano has a broad summit crater, 300 x 400 m wide, containing a central cone.</obo:IAO_0000115>
        <oboInOwl:hasOBONamespace>GAZ</oboInOwl:hasOBONamespace>
        <oboInOwl:id>GAZ:00056324</oboInOwl:id>
        <rdfs:label>Volcan Sumaco</rdfs:label>
    </owl:NamedIndividual>
    


    <!-- http://purl.obolibrary.org/obo/GAZ_00056350 -->

    <owl:NamedIndividual rdf:about="http://purl.obolibrary.org/obo/GAZ_00056350">
        <obo:RO_0001025 rdf:resource="http://purl.obolibrary.org/obo/GAZ_00056362"/>
        <obo:IAO_0000115>A massive ice-covered volcanic complex with at least a half dozen summit cones scattered over a 12 x 20 km area. The 6377 m high summit of the andesitic-to-dacitic complex is a cone at the NW end, north of a line of E-W-trending cones. Deep, steep-walled canyons surrounding the volcano give it an impressive topographic relief of more than 4000 m over a horizontal distance of 15 km. Several young Holocene lava flows descend the NE, SE, and western flanks. The age of its latest eruption is not known, but solfataric activity has been reported.</obo:IAO_0000115>
        <oboInOwl:hasOBONamespace>GAZ</oboInOwl:hasOBONamespace>
        <oboInOwl:id>GAZ:00056350</oboInOwl:id>
        <rdfs:label>Nevado Coropuna</rdfs:label>
    </owl:NamedIndividual>
    


    <!-- http://purl.obolibrary.org/obo/GAZ_00056351 -->

    <owl:NamedIndividual rdf:about="http://purl.obolibrary.org/obo/GAZ_00056351">
        <obo:RO_0001025 rdf:resource="http://purl.obolibrary.org/obo/GAZ_00136449"/>
        <obo:IAO_0000115>A symmetrical andesitic stratovolcano with nested summit craters that towers above the city of Arequipa. The modern symmetrical cone, constructed within a small 1.5 x 2 km wide summit caldera that formed between about 13,700 and 11,300 years ago, caps older Pleistocene volcanoes that underwent caldera collapse about 50,000 years ago. A large scoria cone has grown with the 830-m-wide outer summit crater of El Misti. At least 20 tephra-fall deposits and numerous pyroclastic-flow deposits have been documented during the past 50,000 years, including a pyroclastic flow that traveled 12 km to the south about 2000 years ago. El Misti&apos;s most recent activity has been dominantly pyroclastic, and strong winds have formed a parabolic dune field of volcanic ash extending up to 20 km downwind. An eruption in the 15th century affected Inca inhabitants living near the volcano. Some reports of historical eruptions may represent increased fumarolic activity.</obo:IAO_0000115>
        <oboInOwl:hasOBONamespace>GAZ</oboInOwl:hasOBONamespace>
        <oboInOwl:id>GAZ:00056351</oboInOwl:id>
        <rdfs:label>Volcan El Misti</rdfs:label>
    </owl:NamedIndividual>
    


    <!-- http://purl.obolibrary.org/obo/GAZ_00056352 -->

    <owl:NamedIndividual rdf:about="http://purl.obolibrary.org/obo/GAZ_00056352">
        <obo:RO_0001025 rdf:resource="http://purl.obolibrary.org/obo/GAZ_00136449"/>
        <obo:IAO_0000115>A relatively inconspicuous volcano that was the source of the largest historical eruption of South America in 1600 AD. The volcano has no prominent topographic expression and lies within a 2.5 km wide depression formed by edifice collapse and further excavated by glaciers within an older edifice of Tertiary-to-Pleistocene age. Three overlapping ash cones with craters up to 100 m deep were constructed during the 1600 AD eruption on the floor of the ancestral crater, whose outer flanks are heavily mantled by ash deposits from the 1600 eruption. This powerful fissure-fed eruption may have produced nearly 30 cu km of dacitic tephra, including pyroclastic flows and surges that traveled 13 km to the east and SE. Lahars reached the Pacific Ocean, 120 km away. The eruption caused substantial damage to the major cities of Arequipa and Moquengua, and regional economies took 150 years to fully recover.</obo:IAO_0000115>
        <oboInOwl:hasOBONamespace>GAZ</oboInOwl:hasOBONamespace>
        <oboInOwl:id>GAZ:00056352</oboInOwl:id>
        <rdfs:label>Volcan Huaynaputina</rdfs:label>
    </owl:NamedIndividual>
    


    <!-- http://purl.obolibrary.org/obo/GAZ_00056353 -->

    <owl:NamedIndividual rdf:about="http://purl.obolibrary.org/obo/GAZ_00056353">
        <obo:RO_0001025 rdf:resource="http://purl.obolibrary.org/obo/GAZ_00136449"/>
        <obo:IAO_0000115>A ndesitic-dacitic volcanic complex, located immediately north of Arequipa, consists of a 320 km2 group of Pleistocene lava domes, a stratovolcano complex, and a flank shield volcano. The central, 6057 m high Nevado Chachani complex contains multiple vents along an arcuate line, including a well-defined summit crater at the western end. Two early Pleistocene ignimbrites were erupted from now-buried vents of older edifices. Thin lava flows from Chachani volcano overlie glacial moraines. Pleistocene lava domes form the northern end of the complex. The 8 km wide, late Pleistocene to possibly Holocene lava shield of Pampa de Palacio on the SW side produced a well-preserved lava flow field that represents the youngest products of the Nevado Chachani complex.</obo:IAO_0000115>
        <oboInOwl:hasOBONamespace>GAZ</oboInOwl:hasOBONamespace>
        <oboInOwl:id>GAZ:00056353</oboInOwl:id>
        <rdfs:label>Nevado Chachani Volcanic Complex</rdfs:label>
    </owl:NamedIndividual>
    


    <!-- http://purl.obolibrary.org/obo/GAZ_00056354 -->

    <owl:NamedIndividual rdf:about="http://purl.obolibrary.org/obo/GAZ_00056354">
        <obo:RO_0001025 rdf:resource="http://purl.obolibrary.org/obo/GAZ_00136449"/>
        <obo:IAO_0000115>A stratovolcano.</obo:IAO_0000115>
        <oboInOwl:hasOBONamespace>GAZ</oboInOwl:hasOBONamespace>
        <oboInOwl:id>GAZ:00056354</oboInOwl:id>
        <rdfs:label>Volcan Sabancaya</rdfs:label>
    </owl:NamedIndividual>
    


    <!-- http://purl.obolibrary.org/obo/GAZ_00056355 -->

    <owl:NamedIndividual rdf:about="http://purl.obolibrary.org/obo/GAZ_00056355">
        <obo:RO_0001025 rdf:resource="http://purl.obolibrary.org/obo/GAZ_00136449"/>
        <obo:IAO_0000115>An active stratovolcano. The northernmost of three young volcanoes located along a regional structural lineament about 50 km behind the main volcanic front of Peru. The growth and destruction of Ubinas I volcano was followed by construction of Ubinas II volcano beginning in the mid-Pleistocene. The upper slopes of the andesitic-to-rhyolitic Ubinas II stratovolcano are composed primarily of andesitic and trachyandesitic lava flows and steepen to nearly 45 degrees. The steep-walled, 150-m-deep summit caldera contains an ash cone with a 500-m-wide funnel-shaped vent that is 200 m deep. Debris-avalanche deposits from the collapse of the SE flank of Ubinas about 3700 years ago extend 10 km from the volcano. Widespread plinian pumice-fall deposits from Ubinas include one of Holocene age about 1000 years ago. Holocene lava flows are visible on the volcano&apos;s flanks, but historical activity, documented since the 16th century, has consisted of intermittent minor-to-moderate explosive eruptions.</obo:IAO_0000115>
        <oboInOwl:hasOBONamespace>GAZ</oboInOwl:hasOBONamespace>
        <oboInOwl:id>GAZ:00056355</oboInOwl:id>
        <rdfs:label>Volcan Ubinas</rdfs:label>
    </owl:NamedIndividual>
    


    <!-- http://purl.obolibrary.org/obo/GAZ_00056357 -->

    <owl:NamedIndividual rdf:about="http://purl.obolibrary.org/obo/GAZ_00056357">
        <obo:RO_0001025 rdf:resource="http://purl.obolibrary.org/obo/GAZ_00056399"/>
        <obo:IAO_0000115>A rhyolitic lava dome.</obo:IAO_0000115>
        <oboInOwl:hasOBONamespace>GAZ</oboInOwl:hasOBONamespace>
        <oboInOwl:id>GAZ:00056357</oboInOwl:id>
        <rdfs:label>Oroscocha</rdfs:label>
    </owl:NamedIndividual>
    


    <!-- http://purl.obolibrary.org/obo/GAZ_00056358 -->

    <owl:NamedIndividual rdf:about="http://purl.obolibrary.org/obo/GAZ_00056358">
        <obo:RO_0001025 rdf:resource="http://purl.obolibrary.org/obo/GAZ_00056399"/>
        <obo:IAO_0000115>A high-potassium andesitic scoria cone surrounded by a compound lava shield.</obo:IAO_0000115>
        <oboInOwl:hasOBONamespace>GAZ</oboInOwl:hasOBONamespace>
        <oboInOwl:id>GAZ:00056358</oboInOwl:id>
        <rdfs:label>Quimsachata</rdfs:label>
    </owl:NamedIndividual>
    


    <!-- http://purl.obolibrary.org/obo/GAZ_00056359 -->

    <owl:NamedIndividual rdf:about="http://purl.obolibrary.org/obo/GAZ_00056359">
        <obo:RO_0001025 rdf:resource="http://purl.obolibrary.org/obo/GAZ_00136449"/>
        <obo:IAO_0000115>A cinder cone that lies about 30 km NE of Sara Sara volcano. Along with other, older cones, it is perched on an isolated high plateau far from the nearest roads, east of the Rio Ocona. The Cerro Auquihuato cinder cone was constructed along the southern rim of the plateau and fed a pristine lava flow with very prominent levees that traveled southward down a river valley dissecting the margins of the plateau.</obo:IAO_0000115>
        <oboInOwl:hasOBONamespace>GAZ</oboInOwl:hasOBONamespace>
        <oboInOwl:id>GAZ:00056359</oboInOwl:id>
        <rdfs:label>Cerro Auquihuato</rdfs:label>
    </owl:NamedIndividual>
    


    <!-- http://purl.obolibrary.org/obo/GAZ_00056360 -->

    <owl:NamedIndividual rdf:about="http://purl.obolibrary.org/obo/GAZ_00056360">
        <obo:RO_0001025 rdf:resource="http://purl.obolibrary.org/obo/GAZ_00136449"/>
        <obo:IAO_0000115>A stratovolcano lying between Laguna Parinacocha and the Rio Ocona is the westernmost young volcano in Peru. The 5522 m high andesitic stratovolcano was the source of youthful-looking lava flows with prominent levees that traveled about 10 km eastward into the Rio Ocona valley. Pristine lava flows on the upper slopes of the volcano and ash layers in peat deposits at its base suggest a very young, probably Holocene age.</obo:IAO_0000115>
        <oboInOwl:hasOBONamespace>GAZ</oboInOwl:hasOBONamespace>
        <oboInOwl:id>GAZ:00056360</oboInOwl:id>
        <rdfs:label>Volcan Sara Sara</rdfs:label>
    </owl:NamedIndividual>
    


    <!-- http://purl.obolibrary.org/obo/GAZ_00056361 -->

    <owl:NamedIndividual rdf:about="http://purl.obolibrary.org/obo/GAZ_00056361">
        <obo:IAO_0000115>A lake.</obo:IAO_0000115>
        <oboInOwl:hasOBONamespace>GAZ</oboInOwl:hasOBONamespace>
        <oboInOwl:id>GAZ:00056361</oboInOwl:id>
        <rdfs:label>Laguna Parinacocha</rdfs:label>
    </owl:NamedIndividual>
    


    <!-- http://purl.obolibrary.org/obo/GAZ_00056362 -->

    <owl:NamedIndividual rdf:about="http://purl.obolibrary.org/obo/GAZ_00056362">
        <obo:RO_0001025 rdf:resource="http://purl.obolibrary.org/obo/GAZ_00136449"/>
        <obo:IAO_0000115>A volcanic field in the Andahua valley area, 20 km ENE of Nevados de Coropuna, is a large 60 x 60 km scoria cone and lava field. Known locally as the &quot;Valley of the Volcanoes,&quot; the volcanic field lies in a series of deep NNW-SSE-trending, on echelon valleys: Orcopampa, Andahua and Ayo. The volcanic field contains extremely youthful dominantly trachyandesitic cinder cones and lava flows that have destroyed buildings and may be only a few hundred years old. The area was reported to have been active during the time of the Incas and to have &quot;become active again&quot; in 1913. Lava flows have repeatedly dammed the Rio Andagua valley, and an existing small lake was impounded by the youngest lavas.</obo:IAO_0000115>
        <oboInOwl:hasOBONamespace>GAZ</oboInOwl:hasOBONamespace>
        <oboInOwl:id>GAZ:00056362</oboInOwl:id>
        <rdfs:label>Andahua-Orcopampa Volcanic Field</rdfs:label>
    </owl:NamedIndividual>
    


    <!-- http://purl.obolibrary.org/obo/GAZ_00056363 -->

    <owl:NamedIndividual rdf:about="http://purl.obolibrary.org/obo/GAZ_00056363">
        <obo:RO_0001025 rdf:resource="http://purl.obolibrary.org/obo/GAZ_00136449"/>
        <obo:IAO_0000115>A volcanic field that lies SSE of the Andahua-Orcocampo volcanic field, west of Sabancaya volcano. The Huambo volcanic field is divided into two segments. The southern area contains several cinder cones and associated lava flows, some of which are inferred to be of early to late-Holocene age on the basis of morphological criteria. The northern part contains a single vent, the Cerro Keyocc cinder cone, which produced an extensive lava field that blanketed a plateau to the west during an eruption radiocarbon dated at about 2650 years ago.</obo:IAO_0000115>
        <oboInOwl:hasOBONamespace>GAZ</oboInOwl:hasOBONamespace>
        <oboInOwl:id>GAZ:00056363</oboInOwl:id>
        <rdfs:label>Huambo Volcanic Field</rdfs:label>
    </owl:NamedIndividual>
    


    <!-- http://purl.obolibrary.org/obo/GAZ_00056364 -->

    <owl:NamedIndividual rdf:about="http://purl.obolibrary.org/obo/GAZ_00056364">
        <obo:RO_0001025 rdf:resource="http://purl.obolibrary.org/obo/GAZ_00056365"/>
        <obo:IAO_0000115>A stratovolcano.</obo:IAO_0000115>
        <oboInOwl:hasOBONamespace>GAZ</oboInOwl:hasOBONamespace>
        <oboInOwl:id>GAZ:00056364</oboInOwl:id>
        <rdfs:label>Nevado Sabancaya</rdfs:label>
    </owl:NamedIndividual>
    


    <!-- http://purl.obolibrary.org/obo/GAZ_00056365 -->

    <owl:NamedIndividual rdf:about="http://purl.obolibrary.org/obo/GAZ_00056365">
        <obo:RO_0001025 rdf:resource="http://purl.obolibrary.org/obo/GAZ_00136449"/>
        <obo:IAO_0000115>A stratovolcanic group. Sabancaya, located on the saddle between 6288 m high Ampato and 6025 m high Hualca Hualca volcanoes, is the youngest of these volcanic centers and the only one to have erupted in historical time. The oldest of the three volcanoes, Nevado Hualca Hualca, is of probable late-Pliocene to early Pleistocene age. Both Nevado Ampato and Nevado Sabancaya are only slightly affected by glacial erosion and consist of a series of lava domes aligned along a NW-SW trend.</obo:IAO_0000115>
        <oboInOwl:hasOBONamespace>GAZ</oboInOwl:hasOBONamespace>
        <oboInOwl:id>GAZ:00056365</oboInOwl:id>
        <rdfs:label>Sabancaya Volcanic Group</rdfs:label>
    </owl:NamedIndividual>
    


    <!-- http://purl.obolibrary.org/obo/GAZ_00056366 -->

    <owl:NamedIndividual rdf:about="http://purl.obolibrary.org/obo/GAZ_00056366">
        <obo:RO_0001025 rdf:resource="http://purl.obolibrary.org/obo/GAZ_00056365"/>
        <obo:IAO_0000115>A stratovolcano.</obo:IAO_0000115>
        <oboInOwl:hasOBONamespace>GAZ</oboInOwl:hasOBONamespace>
        <oboInOwl:id>GAZ:00056366</oboInOwl:id>
        <rdfs:label>Nevado Hualca Hualca</rdfs:label>
    </owl:NamedIndividual>
    


    <!-- http://purl.obolibrary.org/obo/GAZ_00056367 -->

    <owl:NamedIndividual rdf:about="http://purl.obolibrary.org/obo/GAZ_00056367">
        <obo:RO_0001025 rdf:resource="http://purl.obolibrary.org/obo/GAZ_00056365"/>
        <obo:IAO_0000115>A stratovolcano.</obo:IAO_0000115>
        <oboInOwl:hasOBONamespace>GAZ</oboInOwl:hasOBONamespace>
        <oboInOwl:id>GAZ:00056367</oboInOwl:id>
        <rdfs:label>Nevado Ampato</rdfs:label>
    </owl:NamedIndividual>
    


    <!-- http://purl.obolibrary.org/obo/GAZ_00056368 -->

    <owl:NamedIndividual rdf:about="http://purl.obolibrary.org/obo/GAZ_00056368">
        <obo:RO_0001025 rdf:resource="http://purl.obolibrary.org/obo/GAZ_00136449"/>
        <obo:IAO_0000115>A small isolated scoria cone, constructed on a plain WSW of Chachani volcano and WNW of El Misti volcano. Andesitic bombs surround the crater of this relatively young volcanic feature that displays a well-preserved crater at the summit of the scoria cone and has a morphology similar to the Holocene Andahua scoria cones farther to the north. Cerro Nicholson was erupted through a 1.65-million-year-old Arequipa Airport Ignimbrite deposit erupted from a now-buried site beneath the Chachani volcanic complex.</obo:IAO_0000115>
        <oboInOwl:hasOBONamespace>GAZ</oboInOwl:hasOBONamespace>
        <oboInOwl:id>GAZ:00056368</oboInOwl:id>
        <rdfs:label>Cerro Nicholson</rdfs:label>
    </owl:NamedIndividual>
    


    <!-- http://purl.obolibrary.org/obo/GAZ_00056369 -->

    <owl:NamedIndividual rdf:about="http://purl.obolibrary.org/obo/GAZ_00056369">
        <obo:RO_0001025 rdf:resource="http://purl.obolibrary.org/obo/GAZ_00136449"/>
        <obo:IAO_0000115>A 5408 m high dacitic lava dome complex in the Ichuna district across the Rio Tambo about 30 km SE of Huaynaputina volcano. Volcan Ticsani resembles Huaynaputina in its dacitic composition and explosive eruptive style. Both volcanoes lie about 50 km behind the main volcanic front of the Peruvian Andes. A fresh-looking lava field lies at the NW base of the youthful-looking, unglaciated volcano. A major debris avalanche produced by collapse of the volcano partially filled the Rio Tambor to the south. The most recent eruptions from Ticsani produced a pumice-fall deposit that extends to the east and a fissure-fed lava dome. No historical eruptions are known from Ticsani, but fumarolic activity continues.</obo:IAO_0000115>
        <oboInOwl:hasOBONamespace>GAZ</oboInOwl:hasOBONamespace>
        <oboInOwl:id>GAZ:00056369</oboInOwl:id>
        <rdfs:label>Ticsani Lava Dome</rdfs:label>
    </owl:NamedIndividual>
    


    <!-- http://purl.obolibrary.org/obo/GAZ_00056370 -->

    <owl:NamedIndividual rdf:about="http://purl.obolibrary.org/obo/GAZ_00056370">
        <obo:RO_0001025 rdf:resource="http://purl.obolibrary.org/obo/GAZ_00136449"/>
        <obo:IAO_0000115>A stratovolcano that consists of two dissected volcanic edifices, of which the southern appears more youthful. Collapse of the northern edifice produced a debris avalanche that traveled 7 km to the north. Postglacial lava flows are present, the largest of which originated from the saddle between the two edifices.</obo:IAO_0000115>
        <oboInOwl:hasOBONamespace>GAZ</oboInOwl:hasOBONamespace>
        <oboInOwl:id>GAZ:00056370</oboInOwl:id>
        <rdfs:label>Volcan Tutupaca</rdfs:label>
    </owl:NamedIndividual>
    


    <!-- http://purl.obolibrary.org/obo/GAZ_00056371 -->

    <owl:NamedIndividual rdf:about="http://purl.obolibrary.org/obo/GAZ_00056371">
        <obo:RO_0001025 rdf:resource="http://purl.obolibrary.org/obo/GAZ_00136449"/>
        <obo:IAO_0000115>An andesitic stratovolcano that has a youthful, well-preserved summit crater. Late-Pleistocene and Holocene eruptions have produced airfall deposits, pyroclastic flows and surges, and block-and-ash flows produced by growth and collapse of lava domes. The most recent plinian eruption took place from Yucamane about 3300 radiocarbon years ago.</obo:IAO_0000115>
        <oboInOwl:hasOBONamespace>GAZ</oboInOwl:hasOBONamespace>
        <oboInOwl:id>GAZ:00056371</oboInOwl:id>
        <rdfs:label>Volcan Yucamane</rdfs:label>
    </owl:NamedIndividual>
    


    <!-- http://purl.obolibrary.org/obo/GAZ_00056372 -->

    <owl:NamedIndividual rdf:about="http://purl.obolibrary.org/obo/GAZ_00056372">
        <obo:RO_0001025 rdf:resource="http://purl.obolibrary.org/obo/GAZ_00136449"/>
        <obo:IAO_0000115>A volcano to the N of Volcan Yucamane.</obo:IAO_0000115>
        <oboInOwl:hasOBONamespace>GAZ</oboInOwl:hasOBONamespace>
        <oboInOwl:id>GAZ:00056372</oboInOwl:id>
        <rdfs:label>Cerro Caliente</rdfs:label>
    </owl:NamedIndividual>
    


    <!-- http://purl.obolibrary.org/obo/GAZ_00056373 -->

    <owl:NamedIndividual rdf:about="http://purl.obolibrary.org/obo/GAZ_00056373">
        <rdf:type rdf:resource="http://purl.obolibrary.org/obo/ENVO_00000354"/>
        <obo:RO_0001025 rdf:resource="http://purl.obolibrary.org/obo/GAZ_00136449"/>
        <obo:IAO_0000115>A volcanic complex that lies near the Chilean border, about 25 km north of Tacora volcano. Nevados Casiri consists of four volcanic edifices, with the youngest cone on the SE side. This compound trachytic and trachyandesitic volcano reaches an elevation of 5650 m and is also known as Paugarani. Two fresh Holocene lava flows are located south of the youngest cone, which has a well-defined summit crater. An older lava dome is located to the west. Two sulfur mines have been opened on the NW and SE flanks.</obo:IAO_0000115>
        <oboInOwl:hasOBONamespace>GAZ</oboInOwl:hasOBONamespace>
        <oboInOwl:id>GAZ:00056373</oboInOwl:id>
        <rdfs:label>Nevados Casiri Volcanic Complex</rdfs:label>
    </owl:NamedIndividual>
    


    <!-- http://purl.obolibrary.org/obo/GAZ_00056374 -->

    <owl:NamedIndividual rdf:about="http://purl.obolibrary.org/obo/GAZ_00056374">
        <obo:IAO_0000115>A mountain range of the Andes located in northern Chile, west of Salar de Atacama. It runs north-south, parallel to the main chain. Cordillera Domeyko marks the eastern border of the Atacama Desert.</obo:IAO_0000115>
        <oboInOwl:hasOBONamespace>GAZ</oboInOwl:hasOBONamespace>
        <oboInOwl:id>GAZ:00056374</oboInOwl:id>
        <rdfs:label>Cordillera Domeyko</rdfs:label>
    </owl:NamedIndividual>
    


    <!-- http://purl.obolibrary.org/obo/GAZ_00056387 -->

    <owl:NamedIndividual rdf:about="http://purl.obolibrary.org/obo/GAZ_00056387">
        <obo:RO_0001025 rdf:resource="http://purl.obolibrary.org/obo/GAZ_00004639"/>
        <obo:IAO_0000115>A freshwater lake located in the Chilean Lake District, 96 km northeast of Puerto Montt and 76 km east of Puerto Varas, within the boundaries of the Vicente Perez Rosales National Park.</obo:IAO_0000115>
        <oboInOwl:hasOBONamespace>GAZ</oboInOwl:hasOBONamespace>
        <oboInOwl:id>GAZ:00056387</oboInOwl:id>
        <rdfs:label>Lago Todos los Santos</rdfs:label>
    </owl:NamedIndividual>
    


    <!-- http://purl.obolibrary.org/obo/GAZ_00056391 -->

    <owl:NamedIndividual rdf:about="http://purl.obolibrary.org/obo/GAZ_00056391">
        <obo:RO_0001025 rdf:resource="http://purl.obolibrary.org/obo/GAZ_00056263"/>
        <obo:IAO_0000115>The section of the Cordillera Oriental in Bolivia.</obo:IAO_0000115>
        <oboInOwl:hasOBONamespace>GAZ</oboInOwl:hasOBONamespace>
        <oboInOwl:id>GAZ:00056391</oboInOwl:id>
        <rdfs:label>Cordillera Oriental of Bolivia</rdfs:label>
    </owl:NamedIndividual>
    


    <!-- http://purl.obolibrary.org/obo/GAZ_00056392 -->

    <owl:NamedIndividual rdf:about="http://purl.obolibrary.org/obo/GAZ_00056392">
        <obo:RO_0001025 rdf:resource="http://purl.obolibrary.org/obo/GAZ_00056391"/>
        <obo:IAO_0000115>A subrange of the Cordillera Oriental of Bolivia. It starts in the north of Chuquisaca with the Presto mountain range and ending in the Caiza and Capirenda mountain ranges in Gran Chaco province in the department of Tarija.</obo:IAO_0000115>
        <oboInOwl:hasOBONamespace>GAZ</oboInOwl:hasOBONamespace>
        <oboInOwl:id>GAZ:00056392</oboInOwl:id>
        <rdfs:label>Cordillera Oriental of Bolivia, Meridional</rdfs:label>
    </owl:NamedIndividual>
    


    <!-- http://purl.obolibrary.org/obo/GAZ_00056393 -->

    <owl:NamedIndividual rdf:about="http://purl.obolibrary.org/obo/GAZ_00056393">
        <obo:RO_0001025 rdf:resource="http://purl.obolibrary.org/obo/GAZ_00056391"/>
        <obo:IAO_0000115>The subrange of the Cordillera Oriental of Bolivia, formed entirely by the Cochacamba mountain range, this section crossing the department of Cochacamba forms the Yungas and the Chapare.</obo:IAO_0000115>
        <oboInOwl:hasOBONamespace>GAZ</oboInOwl:hasOBONamespace>
        <oboInOwl:id>GAZ:00056393</oboInOwl:id>
        <rdfs:label>Cordillera Oriental of Bolivia, Central</rdfs:label>
    </owl:NamedIndividual>
    


    <!-- http://purl.obolibrary.org/obo/GAZ_00056394 -->

    <owl:NamedIndividual rdf:about="http://purl.obolibrary.org/obo/GAZ_00056394">
        <obo:RO_0001025 rdf:resource="http://purl.obolibrary.org/obo/GAZ_00056391"/>
        <obo:IAO_0000115>A subrange of the Cordillera Oriental of Bolivia.</obo:IAO_0000115>
        <oboInOwl:hasOBONamespace>GAZ</oboInOwl:hasOBONamespace>
        <oboInOwl:id>GAZ:00056394</oboInOwl:id>
        <rdfs:label>Cordillera Oriental of Bolivia, Septemtrional</rdfs:label>
    </owl:NamedIndividual>
    


    <!-- http://purl.obolibrary.org/obo/GAZ_00056395 -->

    <owl:NamedIndividual rdf:about="http://purl.obolibrary.org/obo/GAZ_00056395">
        <obo:RO_0001025 rdf:resource="http://purl.obolibrary.org/obo/GAZ_00056288"/>
        <obo:IAO_0000115>A Bolivian mountain range that divides the three river basins in the country and also has the second highest peaks in Bolivia. It is rich in minerals and starts in the north with Chaupi Orco and the three Palomanis that were in the south up to Zapaleri, forming a border with Chile and Argentina. The Cordillera Central is divided into three sections.</obo:IAO_0000115>
        <oboInOwl:hasOBONamespace>GAZ</oboInOwl:hasOBONamespace>
        <oboInOwl:id>GAZ:00056395</oboInOwl:id>
        <rdfs:label>Cordillera Central of Bolivia</rdfs:label>
    </owl:NamedIndividual>
    


    <!-- http://purl.obolibrary.org/obo/GAZ_00056396 -->

    <owl:NamedIndividual rdf:about="http://purl.obolibrary.org/obo/GAZ_00056396">
        <obo:RO_0001025 rdf:resource="http://purl.obolibrary.org/obo/GAZ_00056395"/>
        <obo:IAO_0000115>A subrange of the Cordillera Central of Bolivia.</obo:IAO_0000115>
        <oboInOwl:hasOBONamespace>GAZ</oboInOwl:hasOBONamespace>
        <oboInOwl:id>GAZ:00056396</oboInOwl:id>
        <rdfs:label>Cordillera Central of Bolivia, Septentrional</rdfs:label>
    </owl:NamedIndividual>
    


    <!-- http://purl.obolibrary.org/obo/GAZ_00056397 -->

    <owl:NamedIndividual rdf:about="http://purl.obolibrary.org/obo/GAZ_00056397">
        <obo:RO_0001025 rdf:resource="http://purl.obolibrary.org/obo/GAZ_00056395"/>
        <obo:IAO_0000115>A subrange of the Cordillera Central of Bolivia.</obo:IAO_0000115>
        <oboInOwl:hasOBONamespace>GAZ</oboInOwl:hasOBONamespace>
        <oboInOwl:id>GAZ:00056397</oboInOwl:id>
        <rdfs:label>Cordillera Central of Bolivia, Central</rdfs:label>
    </owl:NamedIndividual>
    


    <!-- http://purl.obolibrary.org/obo/GAZ_00056398 -->

    <owl:NamedIndividual rdf:about="http://purl.obolibrary.org/obo/GAZ_00056398">
        <obo:RO_0001025 rdf:resource="http://purl.obolibrary.org/obo/GAZ_00056395"/>
        <obo:IAO_0000115>A subrange of the Cordillera Central of Bolivia.</obo:IAO_0000115>
        <oboInOwl:hasOBONamespace>GAZ</oboInOwl:hasOBONamespace>
        <oboInOwl:id>GAZ:00056398</oboInOwl:id>
        <rdfs:label>Cordillera Central of Bolivia, Meridional</rdfs:label>
    </owl:NamedIndividual>
    


    <!-- http://purl.obolibrary.org/obo/GAZ_00056399 -->

    <owl:NamedIndividual rdf:about="http://purl.obolibrary.org/obo/GAZ_00056399">
        <obo:RO_0001025 rdf:resource="http://purl.obolibrary.org/obo/GAZ_00056261"/>
        <obo:RO_0001025 rdf:resource="http://purl.obolibrary.org/obo/GAZ_00136449"/>
        <obo:IAO_0000115>A group that consists of two late-Pleistocene and Holocene monogenetic volcanoes lie at the foot of the Cordillera Oriental in an isolated area far east of the main volcanic front. Quimsachata is a high-potassium andesitic scoria cone surrounded by a compound lava shield that was erupted in flat terrain along the Vilcanota River about 11,500 years ago. Oroscocha is a rhyolitic lava dome with a short, thick lava flow erupted from a N-S-trending fissure about 6400 years ago.</obo:IAO_0000115>
        <oboInOwl:hasOBONamespace>GAZ</oboInOwl:hasOBONamespace>
        <oboInOwl:id>GAZ:00056399</oboInOwl:id>
        <rdfs:label>Nevados de Quimsachata</rdfs:label>
    </owl:NamedIndividual>
    


    <!-- http://purl.obolibrary.org/obo/GAZ_00056400 -->

    <owl:NamedIndividual rdf:about="http://purl.obolibrary.org/obo/GAZ_00056400">
        <obo:RO_0001025 rdf:resource="http://purl.obolibrary.org/obo/GAZ_00056399"/>
        <obo:IAO_0000115>A volcano.</obo:IAO_0000115>
        <oboInOwl:hasOBONamespace>GAZ</oboInOwl:hasOBONamespace>
        <oboInOwl:id>GAZ:00056400</oboInOwl:id>
        <rdfs:label>Volcan Humarata</rdfs:label>
    </owl:NamedIndividual>
    


    <!-- http://purl.obolibrary.org/obo/GAZ_00056401 -->

    <owl:NamedIndividual rdf:about="http://purl.obolibrary.org/obo/GAZ_00056401">
        <obo:RO_0001025 rdf:resource="http://purl.obolibrary.org/obo/GAZ_00056399"/>
        <obo:IAO_0000115>A stratovolcano.</obo:IAO_0000115>
        <oboInOwl:hasOBONamespace>GAZ</oboInOwl:hasOBONamespace>
        <oboInOwl:id>GAZ:00056401</oboInOwl:id>
        <rdfs:label>Volcan Acotango</rdfs:label>
    </owl:NamedIndividual>
    


    <!-- http://purl.obolibrary.org/obo/GAZ_00056402 -->

    <owl:NamedIndividual rdf:about="http://purl.obolibrary.org/obo/GAZ_00056402">
        <obo:RO_0001025 rdf:resource="http://purl.obolibrary.org/obo/GAZ_00056399"/>
        <obo:IAO_0000115>A volcano.</obo:IAO_0000115>
        <oboInOwl:hasOBONamespace>GAZ</oboInOwl:hasOBONamespace>
        <oboInOwl:id>GAZ:00056402</oboInOwl:id>
        <rdfs:label>Volcan Capurata</rdfs:label>
    </owl:NamedIndividual>
    


    <!-- http://purl.obolibrary.org/obo/GAZ_00056403 -->

    <owl:NamedIndividual rdf:about="http://purl.obolibrary.org/obo/GAZ_00056403">
        <obo:RO_0001025 rdf:resource="http://purl.obolibrary.org/obo/GAZ_00136449"/>
        <obo:IAO_0000115>A stratovolcano in Bolivia.</obo:IAO_0000115>
        <oboInOwl:hasOBONamespace>GAZ</oboInOwl:hasOBONamespace>
        <oboInOwl:id>GAZ:00056403</oboInOwl:id>
        <rdfs:label>Nevado Anallajsi</rdfs:label>
    </owl:NamedIndividual>
    


    <!-- http://purl.obolibrary.org/obo/GAZ_00056404 -->

    <owl:NamedIndividual rdf:about="http://purl.obolibrary.org/obo/GAZ_00056404">
        <obo:RO_0001025 rdf:resource="http://purl.obolibrary.org/obo/GAZ_00136449"/>
        <obo:IAO_0000115>A maar.</obo:IAO_0000115>
        <oboInOwl:hasOBONamespace>GAZ</oboInOwl:hasOBONamespace>
        <oboInOwl:id>GAZ:00056404</oboInOwl:id>
        <rdfs:label>Cerro Columa</rdfs:label>
    </owl:NamedIndividual>
    


    <!-- http://purl.obolibrary.org/obo/GAZ_00056405 -->

    <owl:NamedIndividual rdf:about="http://purl.obolibrary.org/obo/GAZ_00056405">
        <obo:RO_0001025 rdf:resource="http://purl.obolibrary.org/obo/GAZ_00056391"/>
        <obo:RO_0001025 rdf:resource="http://purl.obolibrary.org/obo/GAZ_00136449"/>
        <obo:IAO_0000115>A volcano. It lies just south of La Paz at the eastern edge of the Altiplano.</obo:IAO_0000115>
        <oboInOwl:hasOBONamespace>GAZ</oboInOwl:hasOBONamespace>
        <oboInOwl:id>GAZ:00056405</oboInOwl:id>
        <rdfs:label>Illimani</rdfs:label>
    </owl:NamedIndividual>
    


    <!-- http://purl.obolibrary.org/obo/GAZ_00056406 -->

    <owl:NamedIndividual rdf:about="http://purl.obolibrary.org/obo/GAZ_00056406">
        <obo:RO_0001025 rdf:resource="http://purl.obolibrary.org/obo/GAZ_00136449"/>
        <obo:IAO_0000115>A small stratovolcano that straddles the Chile/Bolivia border. It is the youngest and most southerly of a NE-SW-trending chain of volcanoes. Irruputuncu was constructed within the collapse scarp of a Holocene debris avalanche whose deposit extends to the SW. Subsequent eruptions filled much of this scarp and produced thick, viscous lava flows down the western flank. The summit complex contains two craters, the southernmost of which is fumarolically active.</obo:IAO_0000115>
        <oboInOwl:hasOBONamespace>GAZ</oboInOwl:hasOBONamespace>
        <oboInOwl:id>GAZ:00056406</oboInOwl:id>
        <rdfs:label>Volcan Irruputuncu</rdfs:label>
    </owl:NamedIndividual>
    


    <!-- http://purl.obolibrary.org/obo/GAZ_00056407 -->

    <owl:NamedIndividual rdf:about="http://purl.obolibrary.org/obo/GAZ_00056407">
        <obo:RO_0001025 rdf:resource="http://purl.obolibrary.org/obo/GAZ_00136449"/>
        <obo:IAO_0000115>A stratovolcano in Bolivia. It lies west of Turco and is composed of andesite and dacite.</obo:IAO_0000115>
        <oboInOwl:hasOBONamespace>GAZ</oboInOwl:hasOBONamespace>
        <oboInOwl:id>GAZ:00056407</oboInOwl:id>
        <rdfs:label>Macizo de Larancagua</rdfs:label>
    </owl:NamedIndividual>
    


    <!-- http://purl.obolibrary.org/obo/GAZ_00056408 -->

    <owl:NamedIndividual rdf:about="http://purl.obolibrary.org/obo/GAZ_00056408">
        <obo:RO_0001025 rdf:resource="http://purl.obolibrary.org/obo/GAZ_00120477"/>
        <obo:RO_0001025 rdf:resource="http://purl.obolibrary.org/obo/GAZ_00136449"/>
        <obo:IAO_0000115>A stratovolcano on the southernmost part of the border between Chile and Bolivia. It is located just southwest of Laguna Verde in Bolivia and northwest of Juriques volcano. The Pleistocene Juriques volcano is located immediately to the SE and is capped by a 1.5 km wide summit crater. Archaeological ruins were found on the 5916 m high crater rim of the steep-sided Volcan Licancabur, which maintains constant 30 degree slopes. The shallow freshwater summit lake is 90 m by 70 m wide and has a measured temperature of 6 degrees C, supporting growth of planktonic fauna at nearly 6000 m altitude. Young blocky andesitic lava flows with prominent levees extend up to 6 km down the NW-to-SW flanks; older flows reach up to 15 km from the summit crater and are covered by pyroclastic-flow deposits that extend 12 km. The most recent activity from Licancabur produced flank lava flows.</obo:IAO_0000115>
        <oboInOwl:hasOBONamespace>GAZ</oboInOwl:hasOBONamespace>
        <oboInOwl:id>GAZ:00056408</oboInOwl:id>
        <rdfs:label>Volcan Licancabur</rdfs:label>
    </owl:NamedIndividual>
    


    <!-- http://purl.obolibrary.org/obo/GAZ_00056409 -->

    <owl:NamedIndividual rdf:about="http://purl.obolibrary.org/obo/GAZ_00056409">
        <obo:RO_0001025 rdf:resource="http://purl.obolibrary.org/obo/GAZ_00120477"/>
        <obo:IAO_0000115>A saline lake in the southwest of the altiplano of Bolivia, in the Department of Potosi, Province of Sud Lipez, on the Chilean border at the foot of the volcano Licancabur. Its colour is caused by sediments, containing copper minerals.</obo:IAO_0000115>
        <oboInOwl:hasOBONamespace>GAZ</oboInOwl:hasOBONamespace>
        <oboInOwl:id>GAZ:00056409</oboInOwl:id>
        <rdfs:label>Laguna Verde</rdfs:label>
    </owl:NamedIndividual>
    


    <!-- http://purl.obolibrary.org/obo/GAZ_00056410 -->

    <owl:NamedIndividual rdf:about="http://purl.obolibrary.org/obo/GAZ_00056410">
        <obo:RO_0001025 rdf:resource="http://purl.obolibrary.org/obo/GAZ_00056411"/>
        <obo:IAO_0000115>A stratovolcano in the Cordillera de Lipez in Sud Lipez province of Potosi Department in southwestern Bolivia.</obo:IAO_0000115>
        <oboInOwl:hasOBONamespace>GAZ</oboInOwl:hasOBONamespace>
        <oboInOwl:id>GAZ:00056410</oboInOwl:id>
        <rdfs:label>Cerro Lipez</rdfs:label>
    </owl:NamedIndividual>
    


    <!-- http://purl.obolibrary.org/obo/GAZ_00056411 -->

    <owl:NamedIndividual rdf:about="http://purl.obolibrary.org/obo/GAZ_00056411">
        <obo:IAO_0000115>A mountain range in southern Potosi, Bolivia and northern Argentina, part of the Andes. The range covers an area of 23,404 km2 and runs in a northeast-southwest direction, between the parallels 22degS and 23degS, helping to form the boundary between Bolivia and Argentina. Thus the Cordillera de Lipez is a transverse range in the Andes, between the Cordillera Oriental and the Cordillera Occidental, creating the southern boundary of the Bolivian Altiplano.</obo:IAO_0000115>
        <oboInOwl:hasOBONamespace>GAZ</oboInOwl:hasOBONamespace>
        <oboInOwl:id>GAZ:00056411</oboInOwl:id>
        <rdfs:label>Cordillera de Lipez</rdfs:label>
    </owl:NamedIndividual>
    


    <!-- http://purl.obolibrary.org/obo/GAZ_00056412 -->

    <owl:NamedIndividual rdf:about="http://purl.obolibrary.org/obo/GAZ_00056412">
        <obo:RO_0001025 rdf:resource="http://purl.obolibrary.org/obo/GAZ_00136449"/>
        <obo:IAO_0000115>A Cenozoic stratovolcano, lava dome and a lava flow complex between Potosi and Uyuni, Bolivia, in the Andes rising to a peak at 5,438 m.</obo:IAO_0000115>
        <oboInOwl:hasOBONamespace>GAZ</oboInOwl:hasOBONamespace>
        <oboInOwl:id>GAZ:00056412</oboInOwl:id>
        <rdfs:label>Volcan Nuevo Mundo</rdfs:label>
    </owl:NamedIndividual>
    


    <!-- http://purl.obolibrary.org/obo/GAZ_00056413 -->

    <owl:NamedIndividual rdf:about="http://purl.obolibrary.org/obo/GAZ_00056413">
        <obo:RO_0001025 rdf:resource="http://purl.obolibrary.org/obo/GAZ_00056764"/>
        <obo:IAO_0000115>A stratovolcano on the border of Chile and Bolivia. It lies in the middle of a 15 km long ridge composed of several stratovolcanos.</obo:IAO_0000115>
        <oboInOwl:hasOBONamespace>GAZ</oboInOwl:hasOBONamespace>
        <oboInOwl:id>GAZ:00056413</oboInOwl:id>
        <rdfs:label>Volcan Olca</rdfs:label>
    </owl:NamedIndividual>
    


    <!-- http://purl.obolibrary.org/obo/GAZ_00056414 -->

    <owl:NamedIndividual rdf:about="http://purl.obolibrary.org/obo/GAZ_00056414">
        <obo:RO_0001025 rdf:resource="http://purl.obolibrary.org/obo/GAZ_00136449"/>
        <obo:IAO_0000115>A massive andesite stratovolcano in the Andes on the border between Bolivia and Chile. It is located southeast of the village that shares its name.</obo:IAO_0000115>
        <oboInOwl:hasOBONamespace>GAZ</oboInOwl:hasOBONamespace>
        <oboInOwl:id>GAZ:00056414</oboInOwl:id>
        <rdfs:label>Volcan Ollague</rdfs:label>
    </owl:NamedIndividual>
    


    <!-- http://purl.obolibrary.org/obo/GAZ_00056416 -->

    <owl:NamedIndividual rdf:about="http://purl.obolibrary.org/obo/GAZ_00056416">
        <obo:RO_0001025 rdf:resource="http://purl.obolibrary.org/obo/GAZ_00136449"/>
        <obo:IAO_0000115>A stratovolcano in Bolivia.</obo:IAO_0000115>
        <oboInOwl:hasOBONamespace>GAZ</oboInOwl:hasOBONamespace>
        <oboInOwl:id>GAZ:00056416</oboInOwl:id>
        <rdfs:label>Macizo de Pacuni</rdfs:label>
    </owl:NamedIndividual>
    


    <!-- http://purl.obolibrary.org/obo/GAZ_00056417 -->

    <owl:NamedIndividual rdf:about="http://purl.obolibrary.org/obo/GAZ_00056417">
        <obo:RO_0001025 rdf:resource="http://purl.obolibrary.org/obo/GAZ_00136449"/>
        <obo:IAO_0000115>A volcanic field that consists of a 45 x 45 km area of coalesced lava flows at the SW margin of Bolivia&apos;s Salar de Uyuni, east of the Andean volcanic front. Several generations of lava flows and cones are present, but the youngest flows are Holocene in age. The young lava field partially or completely surrounds the older dissected stratovolcanoes of Cerro Luxsar and Cerro Uquila.</obo:IAO_0000115>
        <oboInOwl:hasOBONamespace>GAZ</oboInOwl:hasOBONamespace>
        <oboInOwl:id>GAZ:00056417</oboInOwl:id>
        <rdfs:label>Pampa Luxsar Volcanic Field</rdfs:label>
    </owl:NamedIndividual>
    


    <!-- http://purl.obolibrary.org/obo/GAZ_00056418 -->

    <owl:NamedIndividual rdf:about="http://purl.obolibrary.org/obo/GAZ_00056418">
        <obo:RO_0001025 rdf:resource="http://purl.obolibrary.org/obo/GAZ_00056425"/>
        <obo:RO_0001025 rdf:resource="http://purl.obolibrary.org/obo/GAZ_00136449"/>
        <obo:IAO_0000115>A north-south trending complex of volcanos on the border of Bolivia and Chile. It contains two peaks, Pomerape to the north and Parinacota to the south. Parinacota is dormant, having erupted within the last 2000 years, and Pomerape is of Pleistocene age.</obo:IAO_0000115>
        <oboInOwl:hasOBONamespace>GAZ</oboInOwl:hasOBONamespace>
        <oboInOwl:id>GAZ:00056418</oboInOwl:id>
        <rdfs:label>Nevados de Payachata</rdfs:label>
    </owl:NamedIndividual>
    


    <!-- http://purl.obolibrary.org/obo/GAZ_00056419 -->

    <owl:NamedIndividual rdf:about="http://purl.obolibrary.org/obo/GAZ_00056419">
        <obo:RO_0001025 rdf:resource="http://purl.obolibrary.org/obo/GAZ_00056418"/>
        <obo:IAO_0000115>A massive stratovolcano on the border of Chile and Bolivia. It is the southernmost and youngest of a pair of volcanoes forming the Nevados de Payachata volcanic group along the Chile-Bolivia border. The symmetrical, 6348 m high Parinacota volcano forms a twin volcano with the dominantly Pleistocene, 6222 m high Pomerape volcano, which towers above a low saddle to the NE. Collapse of Parinacota about 8000 years ago produced a 6 cu km debris avalanche that traveled 22 km to the west and blocked drainages, forming Lake Chungara. Holocene eruptive activity has subsequently reconstructed the Parinacota stratovolcano, which contains a pristine, 300-m-wide summit crater and youthful lava flows on the western flanks.</obo:IAO_0000115>
        <oboInOwl:hasOBONamespace>GAZ</oboInOwl:hasOBONamespace>
        <oboInOwl:id>GAZ:00056419</oboInOwl:id>
        <rdfs:label>Volcan Parinacota</rdfs:label>
    </owl:NamedIndividual>
    


    <!-- http://purl.obolibrary.org/obo/GAZ_00056420 -->

    <owl:NamedIndividual rdf:about="http://purl.obolibrary.org/obo/GAZ_00056420">
        <obo:RO_0001025 rdf:resource="http://purl.obolibrary.org/obo/GAZ_00056418"/>
        <obo:IAO_0000115>A Pleistocene stratovolcano lying on the border of Chile and Bolivia.</obo:IAO_0000115>
        <oboInOwl:hasOBONamespace>GAZ</oboInOwl:hasOBONamespace>
        <oboInOwl:id>GAZ:00056420</oboInOwl:id>
        <rdfs:label>Volcan Pomerape</rdfs:label>
    </owl:NamedIndividual>
    


    <!-- http://purl.obolibrary.org/obo/GAZ_00056421 -->

    <owl:NamedIndividual rdf:about="http://purl.obolibrary.org/obo/GAZ_00056421">
        <obo:RO_0001025 rdf:resource="http://purl.obolibrary.org/obo/GAZ_00136449"/>
        <obo:IAO_0000115>A stratovolcano in Bolivia.</obo:IAO_0000115>
        <oboInOwl:hasOBONamespace>GAZ</oboInOwl:hasOBONamespace>
        <oboInOwl:id>GAZ:00056421</oboInOwl:id>
        <rdfs:label>Volcan Patilla Pata</rdfs:label>
    </owl:NamedIndividual>
    


    <!-- http://purl.obolibrary.org/obo/GAZ_00056422 -->

    <owl:NamedIndividual rdf:about="http://purl.obolibrary.org/obo/GAZ_00056422">
        <obo:RO_0001025 rdf:resource="http://purl.obolibrary.org/obo/GAZ_00136449"/>
        <obo:IAO_0000115>A low pyroclastic shield near the Rio Lauca on the Bolivian Altiplano. The extremely youthful-looking volcanic complex displays fumarolic activity and is estimated to be of Holocene age. Tambo Quemado consists of a broad ignimbrite shield capped by an elongated NNE-SSW-trending vent area about 2 x 3.5 km in diameter formed by three large overlapping craters. The youngest crater lies at the southern end of the 4215 m high summit region and contains a blocky lava dome. Wind has redistributed tephra deposits to the east and south, forming aeolian sand dunes.</obo:IAO_0000115>
        <oboInOwl:hasOBONamespace>GAZ</oboInOwl:hasOBONamespace>
        <oboInOwl:id>GAZ:00056422</oboInOwl:id>
        <rdfs:label>Sacabaya Pyroclastic Shield</rdfs:label>
    </owl:NamedIndividual>
    


    <!-- http://purl.obolibrary.org/obo/GAZ_00056423 -->

    <owl:NamedIndividual rdf:about="http://purl.obolibrary.org/obo/GAZ_00056423">
        <obo:RO_0001025 rdf:resource="http://purl.obolibrary.org/obo/GAZ_00136449"/>
        <obo:IAO_0000115>A series of volcanoes straddling the border between Bolivia and Chile. It contains at least 10 postglacial centers and stretches from Escalante volcano on the north to Sairecabur volcano on the south. Nomenclature reflecting local usage results in conflicting names applied to these features on Chilean and Bolivian topographic maps. The highest peak, Sairecabur, is located on the northern margin of a 4.5 km wide caldera. Postglacial activity began south of the summit, but most recently produced a pristine lava flow to the NW. An active sulfur mine is located north of the volcano. Escalante, slightly older than Sairecabur, has a crater lake at its summit and youthful lava flows on its flanks, and other eruptive centers have also produced Holocene lava flows. Curinquinca volcano of Pleistocene-Holocene age lies at the NE end of the complex and Cerro Colorado volcano at the NW end.</obo:IAO_0000115>
        <oboInOwl:hasOBONamespace>GAZ</oboInOwl:hasOBONamespace>
        <oboInOwl:id>GAZ:00056423</oboInOwl:id>
        <rdfs:label>Sairecabur Volcanic Complex</rdfs:label>
    </owl:NamedIndividual>
    


    <!-- http://purl.obolibrary.org/obo/GAZ_00056424 -->

    <owl:NamedIndividual rdf:about="http://purl.obolibrary.org/obo/GAZ_00056424">
        <obo:RO_0001025 rdf:resource="http://purl.obolibrary.org/obo/GAZ_00056423"/>
        <oboInOwl:hasOBONamespace>GAZ</oboInOwl:hasOBONamespace>
        <oboInOwl:id>GAZ:00056424</oboInOwl:id>
        <rdfs:label>Cerro Sairecabur</rdfs:label>
    </owl:NamedIndividual>
    


    <!-- http://purl.obolibrary.org/obo/GAZ_00056425 -->

    <owl:NamedIndividual rdf:about="http://purl.obolibrary.org/obo/GAZ_00056425">
        <obo:IAO_0000115>A national park located in Oruro Department, Bolivia. It borders Lauca National Park in Chile.</obo:IAO_0000115>
        <oboInOwl:hasOBONamespace>GAZ</oboInOwl:hasOBONamespace>
        <oboInOwl:id>GAZ:00056425</oboInOwl:id>
        <rdfs:label>Parque Nacional Sajama National Park</rdfs:label>
    </owl:NamedIndividual>
    


    <!-- http://purl.obolibrary.org/obo/GAZ_00056426 -->

    <owl:NamedIndividual rdf:about="http://purl.obolibrary.org/obo/GAZ_00056426">
        <obo:RO_0001025 rdf:resource="http://purl.obolibrary.org/obo/GAZ_00056425"/>
        <obo:RO_0001025 rdf:resource="http://purl.obolibrary.org/obo/GAZ_00136449"/>
        <obo:IAO_0000115>An extinct stratovolcano and the highest peak in Bolivia.</obo:IAO_0000115>
        <oboInOwl:hasOBONamespace>GAZ</oboInOwl:hasOBONamespace>
        <oboInOwl:id>GAZ:00056426</oboInOwl:id>
        <rdfs:label>Nevado Sajama</rdfs:label>
    </owl:NamedIndividual>
    


    <!-- http://purl.obolibrary.org/obo/GAZ_00056427 -->

    <owl:NamedIndividual rdf:about="http://purl.obolibrary.org/obo/GAZ_00056427">
        <obo:RO_0001025 rdf:resource="http://purl.obolibrary.org/obo/GAZ_00136449"/>
        <obo:IAO_0000115>A stratovolcano towers above the northern end of the Salar de Coipasa in the Altiplano of Bolivia. A pyroclastic shield capped by lava domes was topped by effusive eruptions that formed an unglaciated andesitic stratovolcano. Collapse of this edifice produced a large late-Pleistocene debris avalanche that swept into the Salar de Coipasa and covered an area of more than 300 km2 south of the volcano, traveling up to 30 km. Tufa deposits on avalanche hummocks in the Salar de Coipasa correspond to a ca. 12,000 year old high stand of the lake. Renewed eruptions during the Holocene constructed lava domes and flows that have restored much of the original edifice, producing the present-day stratovolcano, whose summit is formed by a 5430 m high lava dome. Youthful lava flows extend down the NW and western flanks of the volcano, and pyroclastic-flow deposits from partial collapse of the summit dome extend to the lower SW flank.</obo:IAO_0000115>
        <oboInOwl:hasOBONamespace>GAZ</oboInOwl:hasOBONamespace>
        <oboInOwl:id>GAZ:00056427</oboInOwl:id>
        <rdfs:label>Volcan Tata Sabaya</rdfs:label>
    </owl:NamedIndividual>
    


    <!-- http://purl.obolibrary.org/obo/GAZ_00056428 -->

    <owl:NamedIndividual rdf:about="http://purl.obolibrary.org/obo/GAZ_00056428">
        <rdf:type rdf:resource="http://purl.obolibrary.org/obo/ENVO_00000354"/>
        <obo:RO_0001025 rdf:resource="http://purl.obolibrary.org/obo/GAZ_00136449"/>
        <obo:IAO_0000115>A volcanic complex located along the border between Bolivia and Chile. On its west side lies the rhyolite lava dome called Cerro La Torta. The international border swings around the eastern rim of a 1.4 km wide crater that truncates the summit of Cerros de Tocorpuri; the crater lies wholly within Chile.</obo:IAO_0000115>
        <oboInOwl:hasOBONamespace>GAZ</oboInOwl:hasOBONamespace>
        <oboInOwl:id>GAZ:00056428</oboInOwl:id>
        <rdfs:label>Cerros de Tocorpuri Volcanic Complex</rdfs:label>
    </owl:NamedIndividual>
    


    <!-- http://purl.obolibrary.org/obo/GAZ_00056429 -->

    <owl:NamedIndividual rdf:about="http://purl.obolibrary.org/obo/GAZ_00056429">
        <obo:RO_0001025 rdf:resource="http://purl.obolibrary.org/obo/GAZ_00056428"/>
        <obo:IAO_0000115>A rhyolite lava dome. It erupted from a central vent and is surrounded by a flat-topped surface with wrinkled flow ridges. The flow terminates in steep, talus-covered margins about 150 m high. Lava extrusion was preceded by minor silicic explosive eruptions.</obo:IAO_0000115>
        <oboInOwl:hasOBONamespace>GAZ</oboInOwl:hasOBONamespace>
        <oboInOwl:id>GAZ:00056429</oboInOwl:id>
        <rdfs:label>Cerro La Torta</rdfs:label>
    </owl:NamedIndividual>
    


    <!-- http://purl.obolibrary.org/obo/GAZ_00056430 -->

    <owl:NamedIndividual rdf:about="http://purl.obolibrary.org/obo/GAZ_00056430">
        <obo:RO_0001025 rdf:resource="http://purl.obolibrary.org/obo/GAZ_00056411"/>
        <obo:RO_0001025 rdf:resource="http://purl.obolibrary.org/obo/GAZ_00136449"/>
        <obo:IAO_0000115>A stratovolcano in SW Bolivia that displays fumarolic activity. Andesitic and dacitic lava flows dominate on Uturuncu, and no pyroclastic deposits were observed during recent field work. Although young lava flows display well-preserved flow features, youthful-looking summit lava flows showed evidence of glaciation. Two active sulfur-producing fumarole fields are located near the summit, and large-scale ground deformation was observed beginning in 1992-05 (Pritchard and Simons, 2002), indicating, along with recently detected seismicity, that a magmatic system is still present.</obo:IAO_0000115>
        <oboInOwl:hasOBONamespace>GAZ</oboInOwl:hasOBONamespace>
        <oboInOwl:id>GAZ:00056430</oboInOwl:id>
        <rdfs:label>Volcan Uturuncu</rdfs:label>
    </owl:NamedIndividual>
    


    <!-- http://purl.obolibrary.org/obo/GAZ_00056431 -->

    <owl:NamedIndividual rdf:about="http://purl.obolibrary.org/obo/GAZ_00056431">
        <obo:RO_0001025 rdf:resource="http://purl.obolibrary.org/obo/GAZ_00136449"/>
        <obo:IAO_0000115>A volcano whose summit is a tripoint at which the borders of Argentina, Bolivia and Chile meet. It is part of Potosi Department (Bolivia), Jujuy Province (Argentina), and Antofagasta Region (Chile). The Bolivian portion of the mountain is protected within Eduardo Avaroa Andean Fauna National Reserve. Moreover, it is close to the sector Salar de Tara-Salar de Aguas Calientes of Los Flamencos National Reserve, Chile.</obo:IAO_0000115>
        <oboInOwl:hasOBONamespace>GAZ</oboInOwl:hasOBONamespace>
        <oboInOwl:id>GAZ:00056431</oboInOwl:id>
        <rdfs:label>Volcan Zapaleri</rdfs:label>
    </owl:NamedIndividual>
    


    <!-- http://purl.obolibrary.org/obo/GAZ_00056447 -->

    <owl:NamedIndividual rdf:about="http://purl.obolibrary.org/obo/GAZ_00056447">
        <obo:RO_0001025 rdf:resource="http://purl.obolibrary.org/obo/GAZ_00136449"/>
        <obo:IAO_0000115>A stratovolcano located northeast of the volcanoes Aguas Calientes and Lascar, and southwest of the sector Salar de Pujsa of Los Flamencos National Reserve, in the Antofagasta Region of Chile. The volcano lies on a high plateau called Puna de Atacama. It is a steep-sided andesitic-dacitic volcano with slopes that reach about 45 degrees, forms the highest peak in this part of the northern Andes. Acamarachi, also known as Cerro Pili, is at the SSE end of a small volcanic complex that extends from the neighboring volcano Colachi to the NNW. A large lava dome is located on the north flank of the 6046 m high volcano. A poorly preserved summit crater and the absence of youthful flank lava flows suggest that Acamarachi was largely constructed in pre-Holocene times, although the summit lava flows draping the upper cone were considered to be of Holocene age (Gonzalez-Ferran, 1995).</obo:IAO_0000115>
        <oboInOwl:hasOBONamespace>GAZ</oboInOwl:hasOBONamespace>
        <oboInOwl:id>GAZ:00056447</oboInOwl:id>
        <rdfs:label>Volcan Acamarachi</rdfs:label>
    </owl:NamedIndividual>
    


    <!-- http://purl.obolibrary.org/obo/GAZ_00056451 -->

    <owl:NamedIndividual rdf:about="http://purl.obolibrary.org/obo/GAZ_00056451">
        <obo:RO_0001025 rdf:resource="http://purl.obolibrary.org/obo/GAZ_00136454"/>
        <obo:IAO_0000115>A caldera located west of Lake Argentino and northeast of Peel Fjord in the southern Andes.</obo:IAO_0000115>
        <oboInOwl:hasOBONamespace>GAZ</oboInOwl:hasOBONamespace>
        <oboInOwl:id>GAZ:00056451</oboInOwl:id>
        <rdfs:label>Aguilera Caldera</rdfs:label>
    </owl:NamedIndividual>
    


    <!-- http://purl.obolibrary.org/obo/GAZ_00056452 -->

    <owl:NamedIndividual rdf:about="http://purl.obolibrary.org/obo/GAZ_00056452">
        <obo:IAO_0000115>A national park located in the Andes, in Los Rios and Los Lagos Regions of Chile. It covers 1,068 km2. The Route 215 passes through the park. It connects with the Argentine Route 231 via Cardenal Antonio Samore Pass.</obo:IAO_0000115>
        <oboInOwl:hasOBONamespace>GAZ</oboInOwl:hasOBONamespace>
        <oboInOwl:id>GAZ:00056452</oboInOwl:id>
        <rdfs:label>Parque Nacional Puyehue</rdfs:label>
    </owl:NamedIndividual>
    


    <!-- http://purl.obolibrary.org/obo/GAZ_00056453 -->

    <owl:NamedIndividual rdf:about="http://purl.obolibrary.org/obo/GAZ_00056453">
        <obo:RO_0001025 rdf:resource="http://purl.obolibrary.org/obo/GAZ_00056452"/>
        <obo:RO_0001025 rdf:resource="http://purl.obolibrary.org/obo/GAZ_00136453"/>
        <obo:IAO_0000115>A cluster of late-Pleistocene to Holocene basaltic-to-andesitic scoria cones, maars and small stratovolcanoes covering an area of 380 km2 SE of Lago Puyehue and NE of Lago Rupanco. The most prominent edifice is the small 1990 m high Casablanca stratovolcano of Holocene age, which has a truncated conical profile and produced a major about 2600 radiocarbon years ago. Older late-Pleistocene stratovolcanoes, such as Sarnoso on the SW side and Fiucha on the NW side, are extensively dissected by glaciers. Fissures oriented in four major directions influence the orientation of the cones of the Antillanca complex. Thermal areas are found in scattered locations on the NW side of the complex.</obo:IAO_0000115>
        <oboInOwl:hasOBONamespace>GAZ</oboInOwl:hasOBONamespace>
        <oboInOwl:id>GAZ:00056453</oboInOwl:id>
        <rdfs:label>Antillanca Volcanic Group</rdfs:label>
    </owl:NamedIndividual>
    


    <!-- http://purl.obolibrary.org/obo/GAZ_00056454 -->

    <owl:NamedIndividual rdf:about="http://purl.obolibrary.org/obo/GAZ_00056454">
        <obo:RO_0001025 rdf:resource="http://purl.obolibrary.org/obo/GAZ_00056452"/>
        <obo:RO_0001025 rdf:resource="http://purl.obolibrary.org/obo/GAZ_00136453"/>
        <obo:IAO_0000115>A fissure vents system located in Los Lagos Region of Chile. Although Cordon Caulle is sometimes listed as part of Puyehue volcano, it is tectonically and magmatically distinct from Puyehue.</obo:IAO_0000115>
        <oboInOwl:hasOBONamespace>GAZ</oboInOwl:hasOBONamespace>
        <oboInOwl:id>GAZ:00056454</oboInOwl:id>
        <rdfs:label>Cordon Caulle Fissure Vents</rdfs:label>
    </owl:NamedIndividual>
    


    <!-- http://purl.obolibrary.org/obo/GAZ_00056455 -->

    <owl:NamedIndividual rdf:about="http://purl.obolibrary.org/obo/GAZ_00056455">
        <obo:RO_0001025 rdf:resource="http://purl.obolibrary.org/obo/GAZ_00056452"/>
        <obo:RO_0001025 rdf:resource="http://purl.obolibrary.org/obo/GAZ_00136453"/>
        <obo:IAO_0000115>A flat-topped stratovolcano located in the Andes, on the border of Osorno Province and Ranco Province, southern Chile.</obo:IAO_0000115>
        <oboInOwl:hasOBONamespace>GAZ</oboInOwl:hasOBONamespace>
        <oboInOwl:id>GAZ:00056455</oboInOwl:id>
        <rdfs:label>Volcan Puyehue</rdfs:label>
    </owl:NamedIndividual>
    


    <!-- http://purl.obolibrary.org/obo/GAZ_00056456 -->

    <owl:NamedIndividual rdf:about="http://purl.obolibrary.org/obo/GAZ_00056456">
        <obo:RO_0001025 rdf:resource="http://purl.obolibrary.org/obo/GAZ_00056453"/>
        <obo:IAO_0000115>The highest peak in the Antilanca group.</obo:IAO_0000115>
        <oboInOwl:hasOBONamespace>GAZ</oboInOwl:hasOBONamespace>
        <oboInOwl:id>GAZ:00056456</oboInOwl:id>
        <rdfs:label>Casablanca Volcano</rdfs:label>
    </owl:NamedIndividual>
    


    <!-- http://purl.obolibrary.org/obo/GAZ_00056457 -->

    <owl:NamedIndividual rdf:about="http://purl.obolibrary.org/obo/GAZ_00056457">
        <obo:RO_0001025 rdf:resource="http://purl.obolibrary.org/obo/GAZ_00004639"/>
        <obo:RO_0001025 rdf:resource="http://purl.obolibrary.org/obo/GAZ_00136453"/>
        <obo:IAO_0000115>A stratovolcano in the border between Argentina and Chile near Bariloche, separating two National Parks: Nahuel Huapi in Argentina and Vicente Perez Rosales in Chile. It is covered by seven glaciers (Frias, Alerce, Castano Overo, Manso, Peulla, Casa Pangue y Rio Blanco) and it is 3,491 meters high. Activity dates back to the early Pleistocene, and the most prominent part of the dominantly basaltic-to-andesitic complex is the prominent, glacier-covered Monte Tronador volcano, which formed in three stages during the mid-Pleistocene. The only possible Holocene activity in the volcano group took place SSE of Monte Tronador, where the Fonck cinder cone (also known as Cerro Volcanico) overlies rocks of the Steffen volcano group SE of Tronador. The well-preserved cone was the source of a single andesitic lava flow that postdates the last glacial cycle dating back to 70,000-14,000 years ago and has variously been inferred to be of latest Pleistocene or Holocene age.</obo:IAO_0000115>
        <oboInOwl:hasOBONamespace>GAZ</oboInOwl:hasOBONamespace>
        <oboInOwl:id>GAZ:00056457</oboInOwl:id>
        <rdfs:label>Volcan Tronador</rdfs:label>
    </owl:NamedIndividual>
    


    <!-- http://purl.obolibrary.org/obo/GAZ_00056458 -->

    <owl:NamedIndividual rdf:about="http://purl.obolibrary.org/obo/GAZ_00056458">
        <obo:RO_0001025 rdf:resource="http://purl.obolibrary.org/obo/GAZ_00004639"/>
        <obo:RO_0001025 rdf:resource="http://purl.obolibrary.org/obo/GAZ_00136453"/>
        <obo:IAO_0000115>A stratovolcano lying between the provinces of Osorno and Llanquihue, in Los Lagos Region of Chile. Osorno was constructed over a roughly 250,000-year-old eroded stratovolcano, La Picada, that has a mostly buried 6 km wide caldera. La Picada underlies Osorno on the NE and has postglacial maars and scoria cones. The 2652 m high dominantly basaltic to basaltic-andesite Osorno is one of the most active volcanoes of the southern Chilean Andes. The conical volcano contains two small dacitic lava domes on the NW and SSE flanks. Flank scoria cones and fissure vents, primarily on the west and SW sides, have produced lava flows that reached Lago Llanquihue. Frequent explosive eruptions including pyroclastic flows and surges have occurred during the past 14,000 years. Historical eruptions at Osorno have originated from both summit and flank vents and have produced basaltic and andesitic lava flows that have entered both Llanquihue and Todos los Santos lakes.</obo:IAO_0000115>
        <oboInOwl:hasOBONamespace>GAZ</oboInOwl:hasOBONamespace>
        <oboInOwl:id>GAZ:00056458</oboInOwl:id>
        <rdfs:label>Volcan Osorno</rdfs:label>
    </owl:NamedIndividual>
    


    <!-- http://purl.obolibrary.org/obo/GAZ_00056459 -->

    <owl:NamedIndividual rdf:about="http://purl.obolibrary.org/obo/GAZ_00056459">
        <obo:RO_0001025 rdf:resource="http://purl.obolibrary.org/obo/GAZ_00004639"/>
        <obo:RO_0001025 rdf:resource="http://purl.obolibrary.org/obo/GAZ_00136453"/>
        <obo:IAO_0000115>A snow-capped volcanic chain located in the Andes, in Los Lagos Region of Chile, near Volcan Osorno. A volcanic chain that lies between Lago Rupanco and Lago Todos Los Santos in the Chilean lake district. Volcan Puntiagudo is a late-Pleistocene andesitic stratovolcano with a prominent 2493 m high sharp-peaked summit that results from glacial dissection. An 18 km-long fissure system with more than 40 late-Pleistocene to Holocene basaltic scoria cones and small stratovolcanoes extends to the NE. Lava flows from these centers descend to the NW and SE, in some cases reaching to the shores of the two lakes, forming irregular peninsulas. The only historical eruption occurred in 1850, when ashfall was reported from the Cordon Cenizos chain.</obo:IAO_0000115>
        <oboInOwl:hasOBONamespace>GAZ</oboInOwl:hasOBONamespace>
        <oboInOwl:id>GAZ:00056459</oboInOwl:id>
        <rdfs:label>Puntiagudo-Cordon Cenizos Volcanic Group</rdfs:label>
    </owl:NamedIndividual>
    


    <!-- http://purl.obolibrary.org/obo/GAZ_00056460 -->

    <owl:NamedIndividual rdf:about="http://purl.obolibrary.org/obo/GAZ_00056460">
        <obo:RO_0001025 rdf:resource="http://purl.obolibrary.org/obo/GAZ_00056462"/>
        <obo:RO_0001025 rdf:resource="http://purl.obolibrary.org/obo/GAZ_00136453"/>
        <obo:IAO_0000115>A stratovolcano located in the Bio-Bio Region of Chile, near Sierra Velluda and on the shore of Laguna del Laja.</obo:IAO_0000115>
        <oboInOwl:hasOBONamespace>GAZ</oboInOwl:hasOBONamespace>
        <oboInOwl:id>GAZ:00056460</oboInOwl:id>
        <rdfs:label>Volcan Antuco</rdfs:label>
    </owl:NamedIndividual>
    


    <!-- http://purl.obolibrary.org/obo/GAZ_00056461 -->

    <owl:NamedIndividual rdf:about="http://purl.obolibrary.org/obo/GAZ_00056461">
        <obo:RO_0001025 rdf:resource="http://purl.obolibrary.org/obo/GAZ_00056462"/>
        <obo:RO_0001025 rdf:resource="http://purl.obolibrary.org/obo/GAZ_00136453"/>
        <obo:IAO_0000115>A massive Pleistocene stratovolcano located immediately southwest of the Antuco volcano, in the Bio-Bio Region of Chile. The heavily glaciated mountain has two main summits and is the tallest mountain in Laguna del Laja National Park.</obo:IAO_0000115>
        <oboInOwl:hasOBONamespace>GAZ</oboInOwl:hasOBONamespace>
        <oboInOwl:id>GAZ:00056461</oboInOwl:id>
        <rdfs:label>Sierra Velluda</rdfs:label>
    </owl:NamedIndividual>
    


    <!-- http://purl.obolibrary.org/obo/GAZ_00056462 -->

    <owl:NamedIndividual rdf:about="http://purl.obolibrary.org/obo/GAZ_00056462">
        <obo:IAO_0000115>A national park of Chile located in the Andes. Established 1958-06-25.</obo:IAO_0000115>
        <oboInOwl:hasOBONamespace>GAZ</oboInOwl:hasOBONamespace>
        <oboInOwl:id>GAZ:00056462</oboInOwl:id>
        <rdfs:label>Parque Nacional Laguna del Laja</rdfs:label>
    </owl:NamedIndividual>
    


    <!-- http://purl.obolibrary.org/obo/GAZ_00056463 -->

    <owl:NamedIndividual rdf:about="http://purl.obolibrary.org/obo/GAZ_00056463">
        <obo:RO_0001025 rdf:resource="http://purl.obolibrary.org/obo/GAZ_00056462"/>
        <obo:IAO_0000115>A freshater lake located in the Bio-Bio Region of Chile. The lake borders and gives its name to Laguna del Laja National Park.</obo:IAO_0000115>
        <oboInOwl:hasOBONamespace>GAZ</oboInOwl:hasOBONamespace>
        <oboInOwl:id>GAZ:00056463</oboInOwl:id>
        <rdfs:label>Laguna del Laja</rdfs:label>
    </owl:NamedIndividual>
    


    <!-- http://purl.obolibrary.org/obo/GAZ_00056470 -->

    <owl:NamedIndividual rdf:about="http://purl.obolibrary.org/obo/GAZ_00056470">
        <obo:RO_0001025 rdf:resource="http://purl.obolibrary.org/obo/GAZ_00136453"/>
        <obo:IAO_0000115>A pyroclastic cone with scattered vegetation cover, located west of Hornopiren volcano and southwest of Yate volcano. It lies on the peninsula that borders Reloncavi Estuary, Reloncavi Sound and Gulf of Ancud. The symmetrical cone contains a well-preserved summit crater. A 6 km wide depression breached to the SW mentioned by Gonzalez-Ferran (1995) and a small lava flow from a second pyroclastic cone that was said to travel to the SW through a breach in the SW side of the depression are not prominent on satellite imagery. Volcan Apagado was estimated to be of Holocene age by Gonzalez-Ferran (1995), consistent with its youthful appearance.</obo:IAO_0000115>
        <oboInOwl:hasOBONamespace>GAZ</oboInOwl:hasOBONamespace>
        <oboInOwl:id>GAZ:00056470</oboInOwl:id>
        <rdfs:label>Volcan Apagado</rdfs:label>
    </owl:NamedIndividual>
    


    <!-- http://purl.obolibrary.org/obo/GAZ_00056472 -->

    <owl:NamedIndividual rdf:about="http://purl.obolibrary.org/obo/GAZ_00056472">
        <obo:IAO_0000115>A national park located in the Andes, in Los Lagos Region of Chile. This national park covers about 393 km2. It is bounded by the Reloncavi Estuary on its east and south sides, and by the Reloncavi Sound to the west (excluding a coastal fringe of a few km. To its north lies Chapo Lake.</obo:IAO_0000115>
        <oboInOwl:hasOBONamespace>GAZ</oboInOwl:hasOBONamespace>
        <oboInOwl:id>GAZ:00056472</oboInOwl:id>
        <rdfs:label>Parque Nacional Alerce Andino</rdfs:label>
    </owl:NamedIndividual>
    


    <!-- http://purl.obolibrary.org/obo/GAZ_00056474 -->

    <owl:NamedIndividual rdf:about="http://purl.obolibrary.org/obo/GAZ_00056474">
        <obo:IAO_0000115>A national park located in the Andes, in the Palena Province, in Los Lagos Region of Chile. The park contains 482 km2 of rugged mountains and unspoilt temperate rainforests. This national park borders the north area of Pumalin Park. In the vicinity of the park lie Hornopiren and Yate volcanoes.</obo:IAO_0000115>
        <oboInOwl:hasOBONamespace>GAZ</oboInOwl:hasOBONamespace>
        <oboInOwl:id>GAZ:00056474</oboInOwl:id>
        <rdfs:label>Parque Nacional Hornopiren</rdfs:label>
    </owl:NamedIndividual>
    


    <!-- http://purl.obolibrary.org/obo/GAZ_00056475 -->

    <owl:NamedIndividual rdf:about="http://purl.obolibrary.org/obo/GAZ_00056475">
        <obo:IAO_0000115>A U-shaped valley located in the Andes, in Los Lagos Region of Chile, south of the Vicente Perez Rosales National Park and the east of the Reloncavi Estuary.</obo:IAO_0000115>
        <oboInOwl:hasOBONamespace>GAZ</oboInOwl:hasOBONamespace>
        <oboInOwl:id>GAZ:00056475</oboInOwl:id>
        <rdfs:label>Cochamo Valley</rdfs:label>
    </owl:NamedIndividual>
    


    <!-- http://purl.obolibrary.org/obo/GAZ_00056476 -->

    <owl:NamedIndividual rdf:about="http://purl.obolibrary.org/obo/GAZ_00056476">
        <obo:RO_0001025 rdf:resource="http://purl.obolibrary.org/obo/GAZ_00136454"/>
        <obo:IAO_0000115>A heavily ice-covered volcano located in the Aysen Region of Chile, within Laguna San Rafael National Park. It towers over the southern part of the Northern Patagonian Ice Field.</obo:IAO_0000115>
        <oboInOwl:hasOBONamespace>GAZ</oboInOwl:hasOBONamespace>
        <oboInOwl:id>GAZ:00056476</oboInOwl:id>
        <rdfs:label>Cerro Arenales</rdfs:label>
    </owl:NamedIndividual>
    


    <!-- http://purl.obolibrary.org/obo/GAZ_00056477 -->

    <owl:NamedIndividual rdf:about="http://purl.obolibrary.org/obo/GAZ_00056477">
        <obo:RO_0001025 rdf:resource="http://purl.obolibrary.org/obo/GAZ_00136449"/>
        <obo:IAO_0000115>A stratovolcano located in Arica y Parinacota Region of Chile, near the border with Bolivia. It lies north of the Salar de Surire.</obo:IAO_0000115>
        <oboInOwl:hasOBONamespace>GAZ</oboInOwl:hasOBONamespace>
        <oboInOwl:id>GAZ:00056477</oboInOwl:id>
        <rdfs:label>Volcan Arintica</rdfs:label>
    </owl:NamedIndividual>
    


    <!-- http://purl.obolibrary.org/obo/GAZ_00056478 -->

    <owl:NamedIndividual rdf:about="http://purl.obolibrary.org/obo/GAZ_00056478">
        <obo:RO_0001025 rdf:resource="http://purl.obolibrary.org/obo/GAZ_00136449"/>
        <obo:IAO_0000115>A massive stratovolcano located in Antofagasta Region of northern Chile, just south of the border with Bolivia. Several distinct cones are located along a 10 km-long, E-W-trending ridge that forms the broad summit of the 6176 m high stratovolcano. A Pleistocene debris-avalanche deposit is a prominent feature on the lower NW flank. Extensive Pleistocene glacial moraines surround the volcano. Aucanquilcha presently displays fumarolic activity.</obo:IAO_0000115>
        <oboInOwl:hasOBONamespace>GAZ</oboInOwl:hasOBONamespace>
        <oboInOwl:id>GAZ:00056478</oboInOwl:id>
        <rdfs:label>Cerro Aucanquilcha</rdfs:label>
    </owl:NamedIndividual>
    


    <!-- http://purl.obolibrary.org/obo/GAZ_00056479 -->

    <owl:NamedIndividual rdf:about="http://purl.obolibrary.org/obo/GAZ_00056479">
        <rdf:type rdf:resource="http://purl.obolibrary.org/obo/ENVO_00000354"/>
        <obo:RO_0001025 rdf:resource="http://purl.obolibrary.org/obo/GAZ_00136449"/>
        <obo:IAO_0000115>A volcanic complex located between Salar de Talar and Salar de Capur, in the Antofagasta Region of Chile. More than a half dozen vents produced andesitic-to-dacitic lava flows, with young flows descending to the NE and SE from the 4450 m high summit.</obo:IAO_0000115>
        <oboInOwl:hasOBONamespace>GAZ</oboInOwl:hasOBONamespace>
        <oboInOwl:id>GAZ:00056479</oboInOwl:id>
        <rdfs:label>Caichinque Volcanic Complex</rdfs:label>
    </owl:NamedIndividual>
    


    <!-- http://purl.obolibrary.org/obo/GAZ_00056480 -->

    <owl:NamedIndividual rdf:about="http://purl.obolibrary.org/obo/GAZ_00056480">
        <obo:RO_0001025 rdf:resource="http://purl.obolibrary.org/obo/GAZ_00056481"/>
        <obo:RO_0001025 rdf:resource="http://purl.obolibrary.org/obo/GAZ_00136453"/>
        <obo:IAO_0000115>A stratovolcano in southern Chile, located southeast of Llanquihue Lake and northwest of Chapo Lake, in the Los Lagos Region. The isolated late-Pleistocene to Holocene andesitic volcano rises to 2003 m south of Lake Llanquihue in the Chilean lake district. The 2003 m high Calbuco is elongated in a SW-NE direction and is capped by a 400-500 m wide summit crater. The complex evolution of Calbuco included edifice collapse of an intermediate edifice during the late Pleistocene that produced a 3 cu km debris avalanche that reached the lake. One of the largest historical eruptions in southern Chile took place from Calbuco in 1893-1894 and concluded with lava dome emplacement. Subsequent eruptions have enlarged the lava-dome complex in the summit crater.</obo:IAO_0000115>
        <oboInOwl:hasOBONamespace>GAZ</oboInOwl:hasOBONamespace>
        <oboInOwl:id>GAZ:00056480</oboInOwl:id>
        <rdfs:label>Volcan Calbuco</rdfs:label>
    </owl:NamedIndividual>
    


    <!-- http://purl.obolibrary.org/obo/GAZ_00056481 -->

    <owl:NamedIndividual rdf:about="http://purl.obolibrary.org/obo/GAZ_00056481">
        <obo:IAO_0000115>A protected area.</obo:IAO_0000115>
        <oboInOwl:hasOBONamespace>GAZ</oboInOwl:hasOBONamespace>
        <oboInOwl:id>GAZ:00056481</oboInOwl:id>
        <rdfs:label>Reserva Nacional Llanquihue</rdfs:label>
    </owl:NamedIndividual>
    


    <!-- http://purl.obolibrary.org/obo/GAZ_00056482 -->

    <owl:NamedIndividual rdf:about="http://purl.obolibrary.org/obo/GAZ_00056482">
        <obo:RO_0001025 rdf:resource="http://purl.obolibrary.org/obo/GAZ_00136453"/>
        <obo:IAO_0000115>A stratovolcano located in the Bio-Bio Region of Chile. The late-Pleistocene to Holocene Callaqui stratovolcano has a profile of an overturned canoe due to its construction along an 11 km-long, SW-NE fissure above a 1.2-0.3 million year old Pleistocene edifice. The ice-capped, 3164 m high basaltic-andesite Callaqui volcano contains well-preserved volcanic cones and lava flows, which have traveled up to 14 km. Small craters 100-500 m in diameter are primarily found along a fissure extending down the SW flank. Intense solfataric activity occurs at the southern part of the summit; in 1966 and 1978, red glow was observed in fumarolic areas. Periods of intense fumarolic activity have dominated at Callaqui, and few historical eruptions are known.</obo:IAO_0000115>
        <oboInOwl:hasOBONamespace>GAZ</oboInOwl:hasOBONamespace>
        <oboInOwl:id>GAZ:00056482</oboInOwl:id>
        <rdfs:label>Volcan Callaqui</rdfs:label>
    </owl:NamedIndividual>
    


    <!-- http://purl.obolibrary.org/obo/GAZ_00056483 -->

    <owl:NamedIndividual rdf:about="http://purl.obolibrary.org/obo/GAZ_00056483">
        <obo:RO_0001025 rdf:resource="http://purl.obolibrary.org/obo/GAZ_00136453"/>
        <obo:IAO_0000115>A group of cinder cones in central Chile. The group includes a group of about 50 basaltic to basaltic-andesite scoria cones, maars, and a small stratovolcano that are broadly aligned along a 17 km-long ENE-WSW trend ESE of Lago Ranco. The volcano group occupies a low-lying area north of the more topographically prominent Cordon Caulle-Puyehue volcanic chain, and many of the vents are postglacial in age. The Mirador scoria cone and two maars, Rininahue and Carran, were formed during eruptions in the 20th century. These historical eruptions were concentrated where the regional Liquine-Ofqui fault zone intersects the alignment of volcanic vents.</obo:IAO_0000115>
        <oboInOwl:hasOBONamespace>GAZ</oboInOwl:hasOBONamespace>
        <oboInOwl:id>GAZ:00056483</oboInOwl:id>
        <rdfs:label>Carran-Los Venados Cinder Cones</rdfs:label>
    </owl:NamedIndividual>
    


    <!-- http://purl.obolibrary.org/obo/GAZ_00056484 -->

    <owl:NamedIndividual rdf:about="http://purl.obolibrary.org/obo/GAZ_00056484">
        <obo:RO_0001025 rdf:resource="http://purl.obolibrary.org/obo/GAZ_00136453"/>
        <obo:IAO_0000115>An active stratovolcano located in central Chile, immediately south of Descabezado Grande volcano. Steep-sided 3788 m high Cerro Azul has a 500-m-wide summit crater that is open to the north. The three basaltic-andesite &quot;La Resoloma Craters&quot; scoria vents are located below the west flank and the two &quot;Los Hornitos&quot; scoria cones on the lower SW flank. Quizapu, a major vent on the northern flank of Cerro Azul, formed in 1846 during the first historical eruption at Cerro Azul, accompanied by the emission of voluminous dacitic lava flows that traveled both east into the Estero Barroso valley and west into the Rio Blanquillo valley. Quizapu was later the source of one of the world&apos;s largest explosive eruptions of the 20th century in 1932, which created a 600-700 m wide, 150-m-deep crater and ejected 9.5 cu km of dacitic tephra.</obo:IAO_0000115>
        <oboInOwl:hasOBONamespace>GAZ</oboInOwl:hasOBONamespace>
        <oboInOwl:id>GAZ:00056484</oboInOwl:id>
        <rdfs:label>Cerro Azul</rdfs:label>
    </owl:NamedIndividual>
    


    <!-- http://purl.obolibrary.org/obo/GAZ_00056485 -->

    <owl:NamedIndividual rdf:about="http://purl.obolibrary.org/obo/GAZ_00056485">
        <obo:RO_0001025 rdf:resource="http://purl.obolibrary.org/obo/GAZ_00136449"/>
        <obo:IAO_0000115>A complex volcano on the northern part border between Argentina and Chile. It consists of four overlapping stratovolcanoes along a north-south line. The summit of the complex is located just west of the border in Chile.</obo:IAO_0000115>
        <oboInOwl:hasOBONamespace>GAZ</oboInOwl:hasOBONamespace>
        <oboInOwl:id>GAZ:00056485</oboInOwl:id>
        <rdfs:label>Cerro Bayo</rdfs:label>
    </owl:NamedIndividual>
    


    <!-- http://purl.obolibrary.org/obo/GAZ_00056486 -->

    <owl:NamedIndividual rdf:about="http://purl.obolibrary.org/obo/GAZ_00056486">
        <obo:RO_0001025 rdf:resource="http://purl.obolibrary.org/obo/GAZ_00136449"/>
        <obo:IAO_0000115>A stratovolcano located in El Loa Province, Antofagasta Region, Chile. It is part of a chain of volcanoes that separate Upper Loa River basin from Salar de Ascotan basin and is flanked to the west by a dacitic lava dome called Chanka.</obo:IAO_0000115>
        <oboInOwl:hasOBONamespace>GAZ</oboInOwl:hasOBONamespace>
        <oboInOwl:id>GAZ:00056486</oboInOwl:id>
        <rdfs:label>Cerro del Azufre</rdfs:label>
    </owl:NamedIndividual>
    


    <!-- http://purl.obolibrary.org/obo/GAZ_00056487 -->

    <owl:NamedIndividual rdf:about="http://purl.obolibrary.org/obo/GAZ_00056487">
        <obo:RO_0001025 rdf:resource="http://purl.obolibrary.org/obo/GAZ_00136449"/>
        <obo:IAO_0000115>A stratovolcano located in El Loa Province, Antofagasta Region. It is a 5760 m high andesitic stratovolcano north of Toconce volcano. Cerro del Leon is flanked by two massive dacitic lava domes, 2.6 cu km Chillahuita to the SE and 26 cu km Chao to the NW, in the saddle between Cerro del Leon and Paniri volcanoes. Gonzalez-Ferran (1995) considered El Leon volcano to be of Pleistocene-Holocene age. The massive Chao lava dome and flow is the world&apos;s largest of its type. The 14.5 km-long dacitic lava flow has distal margins that are 350-400 m high and dramatic 30 m high flow ridges on its surface.</obo:IAO_0000115>
        <oboInOwl:hasOBONamespace>GAZ</oboInOwl:hasOBONamespace>
        <oboInOwl:id>GAZ:00056487</oboInOwl:id>
        <rdfs:label>Cerro del Leon</rdfs:label>
    </owl:NamedIndividual>
    


    <!-- http://purl.obolibrary.org/obo/GAZ_00056488 -->

    <owl:NamedIndividual rdf:about="http://purl.obolibrary.org/obo/GAZ_00056488">
        <obo:RO_0001025 rdf:resource="http://purl.obolibrary.org/obo/GAZ_00136449"/>
        <obo:IAO_0000115>A small andesitic-dacitic stratovolcano, has young-looking lava flows and a well-preserved crater. It is the youngest volcanic center of the NW-SE-trending Corrida de Cori range that marks the Chile/Argentina border. Cerro Escorial is located 4 km NE of an active sulfur mine in older, extensively hydrothermally altered rocks. Very youthful-looking lava flows extend westward 3-4 km over an ignimbrite deposit on the Chilean side. A 1 km wide crater caps the summit. Cerro Escorial was considered by de Silva and Francis (1991) to be of probable Holocene age based on morphological evidence, but Richards and Villeneuve (2002) obtained an Ar/Ar age of about 0.342 million years on a lava flow from Cerro Escorial. Most of the lava flows extend to the SW into Chile, but a few small lobes traveled NE on the Argentinian side of the volcano.</obo:IAO_0000115>
        <oboInOwl:hasOBONamespace>GAZ</oboInOwl:hasOBONamespace>
        <oboInOwl:id>GAZ:00056488</oboInOwl:id>
        <rdfs:label>Cerro Escorial</rdfs:label>
    </owl:NamedIndividual>
    


    <!-- http://purl.obolibrary.org/obo/GAZ_00056489 -->

    <owl:NamedIndividual rdf:about="http://purl.obolibrary.org/obo/GAZ_00056489">
        <obo:RO_0001025 rdf:resource="http://purl.obolibrary.org/obo/GAZ_00136453"/>
        <obo:IAO_0000115>A stratovolcano in southern Chile. Cerro Hudson is the southernmost volcano in the Chilean Andes related to subduction of the Nazca plate beneath the South American plate. The massive, 1905 m high Cerro Hudson covers an area of 300 sq km. The compound caldera is drained through a breach on its NW rim, which has been the source of mudflows down the Rio de Los Huemeles. Two cinder cones occur north of the volcano and others occupy the SW and SE flanks. Hudson has been the source of several major Holocene explosive eruptions. An eruption about 6700 years ago was one of the largest known in the southern Andes during the Holocene; another eruption about 3600 years ago also produced more than 10 cu km of tephra. An eruption in 1991 was Chile&apos;s second largest of the 20th century and formed a new 800-m-wide crater in the SW part of the caldera.</obo:IAO_0000115>
        <oboInOwl:hasOBONamespace>GAZ</oboInOwl:hasOBONamespace>
        <oboInOwl:id>GAZ:00056489</oboInOwl:id>
        <rdfs:label>Cerro Hudson</rdfs:label>
    </owl:NamedIndividual>
    


    <!-- http://purl.obolibrary.org/obo/GAZ_00056490 -->

    <owl:NamedIndividual rdf:about="http://purl.obolibrary.org/obo/GAZ_00056490">
        <obo:RO_0001025 rdf:resource="http://purl.obolibrary.org/obo/GAZ_00136453"/>
        <obo:IAO_0000115>A stratovolcano on the border of Argentina and Chile. It lies immediately south of Cardenal Antonio Samore Pass. Cerro Pantoja is an eroded 2024 m high dominantly basaltic volcano of Pleistocene age. Cerro Pantoja lies SSW of Lake Constancia, which is located immediately west of the Argentinian border, and has a dramatic steep-sided summit pinnacle.</obo:IAO_0000115>
        <oboInOwl:hasOBONamespace>GAZ</oboInOwl:hasOBONamespace>
        <oboInOwl:id>GAZ:00056490</oboInOwl:id>
        <rdfs:label>Cerro Pantoja</rdfs:label>
    </owl:NamedIndividual>
    


    <!-- http://purl.obolibrary.org/obo/GAZ_00056491 -->

    <owl:NamedIndividual rdf:about="http://purl.obolibrary.org/obo/GAZ_00056491">
        <obo:RO_0001025 rdf:resource="http://purl.obolibrary.org/obo/GAZ_00056504"/>
        <obo:IAO_0000115>A stratovolcano located in the Antofagasta Region of Chile, immediately north of Cerro Miscanti. The 5778 m high summit contains a 500-m-wide crater. Several youthful lava flows, some of which are considered to be of Holocene age (de Silva and Francis, 1991), descend its flanks. The largest of these extends 5 km to the NW. Older lava flows reach up to 10 km from the summit on the north flank. This volcano had previously been considered to be dormant; however, in 2002 a NASA nighttime thermal infrared satellite image from the Advanced Spaceborne Thermal Emission and Reflection Radiometer (ASTER) showed low-level hot spots in the summit crater and upper flanks. The solitary Holocene Cerro Overo maar is located on the lower NE flank of Chiliques volcano, west of the Salar de Aguas Calientes. The 600-m-wide, 80-m-deep mafic maar produced the least silicic youthful volcanic rocks found in this part of the central Andes.</obo:IAO_0000115>
        <oboInOwl:hasOBONamespace>GAZ</oboInOwl:hasOBONamespace>
        <oboInOwl:id>GAZ:00056491</oboInOwl:id>
        <rdfs:label>Chiliques Volcano</rdfs:label>
    </owl:NamedIndividual>
    


    <!-- http://purl.obolibrary.org/obo/GAZ_00056493 -->

    <owl:NamedIndividual rdf:about="http://purl.obolibrary.org/obo/GAZ_00056493">
        <obo:RO_0001025 rdf:resource="http://purl.obolibrary.org/obo/GAZ_00136453"/>
        <obo:IAO_0000115>An elongated composite cone constructed along the Chile-Argentina border within the 6.5 x 8.5 km wide Trapa-Trapa caldera that formed between 0.6 and 0.4 million years ago near the NW margin of the 20 x 15 km Pliocene Caviahue (Del Agrio) caldera. The eastern summit crater, part of a 2 km-long, ENE-WSW line of nine craters, contains a briny, acidic 300-m-wide crater lake (also referred to as El Agrio or Del Agrio) and displays intense fumarolic activity. Acidic hot springs occur below the eastern outlet of the crater lake, contributing to the acidity of the Rio Agrio, and another geothermal zone is located within Caviahue caldera about 7 km NE of the summit. Infrequent mild-to-moderate explosive eruptions have been recorded at Copahue since the 18th century. Twentieth-century eruptions from the crater lake have ejected pyroclastic rocks and chilled liquid sulfur fragments.</obo:IAO_0000115>
        <oboInOwl:hasOBONamespace>GAZ</oboInOwl:hasOBONamespace>
        <oboInOwl:id>GAZ:00056493</oboInOwl:id>
        <rdfs:label>Volcan Copahue</rdfs:label>
    </owl:NamedIndividual>
    


    <!-- http://purl.obolibrary.org/obo/GAZ_00056494 -->

    <owl:NamedIndividual rdf:about="http://purl.obolibrary.org/obo/GAZ_00056494">
        <obo:IAO_0000115>A national park. It is divided into two zones, the northern zone encompasing the southern portion of Salar de Maricunga and Laguna Santa Rosa, and the southern area the Laguna del Negro Francisco.</obo:IAO_0000115>
        <oboInOwl:hasOBONamespace>GAZ</oboInOwl:hasOBONamespace>
        <oboInOwl:id>GAZ:00056494</oboInOwl:id>
        <rdfs:label>Parque Nacional Nevado Tres Cruces</rdfs:label>
    </owl:NamedIndividual>
    


    <!-- http://purl.obolibrary.org/obo/GAZ_00056495 -->

    <owl:NamedIndividual rdf:about="http://purl.obolibrary.org/obo/GAZ_00056495">
        <rdf:type rdf:resource="http://purl.obolibrary.org/obo/ENVO_00000279"/>
        <obo:RO_0001025 rdf:resource="http://purl.obolibrary.org/obo/GAZ_00056494"/>
        <obo:IAO_0000115>A salt flat located 180 km northeast of the city of Copiapo in the Andes mountains.</obo:IAO_0000115>
        <oboInOwl:hasOBONamespace>GAZ</oboInOwl:hasOBONamespace>
        <oboInOwl:id>GAZ:00056495</oboInOwl:id>
        <rdfs:label>Salar de Maricunga</rdfs:label>
    </owl:NamedIndividual>
    


    <!-- http://purl.obolibrary.org/obo/GAZ_00056496 -->

    <owl:NamedIndividual rdf:about="http://purl.obolibrary.org/obo/GAZ_00056496">
        <obo:RO_0001025 rdf:resource="http://purl.obolibrary.org/obo/GAZ_00056494"/>
        <obo:IAO_0000115>A saline lagoon located just south of the Salar de Maricung. A Ramsar Site.</obo:IAO_0000115>
        <oboInOwl:hasOBONamespace>GAZ</oboInOwl:hasOBONamespace>
        <oboInOwl:id>GAZ:00056496</oboInOwl:id>
        <rdfs:label>Laguna Santa Rosa</rdfs:label>
    </owl:NamedIndividual>
    


    <!-- http://purl.obolibrary.org/obo/GAZ_00056497 -->

    <owl:NamedIndividual rdf:about="http://purl.obolibrary.org/obo/GAZ_00056497">
        <obo:RO_0001025 rdf:resource="http://purl.obolibrary.org/obo/GAZ_00056494"/>
        <obo:IAO_0000115>A saline lagoon located 210 km northeast of Copiapo at 4,126 meters.</obo:IAO_0000115>
        <oboInOwl:hasOBONamespace>GAZ</oboInOwl:hasOBONamespace>
        <oboInOwl:id>GAZ:00056497</oboInOwl:id>
        <rdfs:label>Laguna del Negro Francisco</rdfs:label>
    </owl:NamedIndividual>
    


    <!-- http://purl.obolibrary.org/obo/GAZ_00056498 -->

    <owl:NamedIndividual rdf:about="http://purl.obolibrary.org/obo/GAZ_00056498">
        <obo:RO_0001025 rdf:resource="http://purl.obolibrary.org/obo/GAZ_00056494"/>
        <obo:RO_0001025 rdf:resource="http://purl.obolibrary.org/obo/GAZ_00136449"/>
        <obo:IAO_0000115>A stratovolcano located in the Atacama Region of Chile. The volcano separates the two portions in which Nevado Tres Cruces National Park is divided. In its vicinity lies Ojos del Salado.</obo:IAO_0000115>
        <oboInOwl:hasOBONamespace>GAZ</oboInOwl:hasOBONamespace>
        <oboInOwl:id>GAZ:00056498</oboInOwl:id>
        <rdfs:label>Volcan Copiapo</rdfs:label>
    </owl:NamedIndividual>
    


    <!-- http://purl.obolibrary.org/obo/GAZ_00056499 -->

    <owl:NamedIndividual rdf:about="http://purl.obolibrary.org/obo/GAZ_00056499">
        <obo:RO_0001025 rdf:resource="http://purl.obolibrary.org/obo/GAZ_00136449"/>
        <obo:IAO_0000115>A stratovolcano that rises to 6887 m along the Chile-Argentina border. The volcano lies about 20 km south of the road that crosses the international border at Paso de San Francisco. The summit complex, which is elongated in a NE-SW direction and overlies a largely buried caldera, contains numerous craters, pyroclastic cones and andesitic-to-rhyolitic lava domes and has been the source of Holocene lava flows. A major rhyodacitic explosive eruption took place about 1000-1500 years ago, producing pumiceous pyroclastic flows. The most recent eruptive activity of Ojos del Salado appears to have originated along a NNE-trending rift along the summit complex. It involved formation of a thick, viscous lava flow and at least a dozen small cones, lava domes, and explosion craters.</obo:IAO_0000115>
        <oboInOwl:hasOBONamespace>GAZ</oboInOwl:hasOBONamespace>
        <oboInOwl:id>GAZ:00056499</oboInOwl:id>
        <rdfs:label>Nevados Ojos del Salado</rdfs:label>
    </owl:NamedIndividual>
    


    <!-- http://purl.obolibrary.org/obo/GAZ_00056500 -->

    <owl:NamedIndividual rdf:about="http://purl.obolibrary.org/obo/GAZ_00056500">
        <obo:RO_0001025 rdf:resource="http://purl.obolibrary.org/obo/GAZ_00056501"/>
        <obo:RO_0001025 rdf:resource="http://purl.obolibrary.org/obo/GAZ_00136453"/>
        <obo:IAO_0000115>A stratovolcano located about 25 km south of the mouth of Yelcho River, in the Palena Province, Los Lagos Region, Chile. It was seen in eruption by Darwin. Corcovado, probably of late-Pleistocene age, is eroded by glaciers and surrounded by Holocene cinder cones. A series of lakes flank the eastern side of the basaltic to basaltic-andesite volcano.</obo:IAO_0000115>
        <oboInOwl:hasOBONamespace>GAZ</oboInOwl:hasOBONamespace>
        <oboInOwl:id>GAZ:00056500</oboInOwl:id>
        <rdfs:label>Volcan Corcovado</rdfs:label>
    </owl:NamedIndividual>
    


    <!-- http://purl.obolibrary.org/obo/GAZ_00056501 -->

    <owl:NamedIndividual rdf:about="http://purl.obolibrary.org/obo/GAZ_00056501">
        <obo:IAO_0000115>A national park that is bordered by the gulf of the same name to the west. The park includes the volcanoes Corcovado and Yanteles.</obo:IAO_0000115>
        <oboInOwl:hasOBONamespace>GAZ</oboInOwl:hasOBONamespace>
        <oboInOwl:id>GAZ:00056501</oboInOwl:id>
        <rdfs:label>Parque Nacional Corcovado</rdfs:label>
    </owl:NamedIndividual>
    


    <!-- http://purl.obolibrary.org/obo/GAZ_00056502 -->

    <owl:NamedIndividual rdf:about="http://purl.obolibrary.org/obo/GAZ_00056502">
        <obo:RO_0001025 rdf:resource="http://purl.obolibrary.org/obo/GAZ_00056501"/>
        <obo:RO_0001025 rdf:resource="http://purl.obolibrary.org/obo/GAZ_00136453"/>
        <obo:IAO_0000115>A stratovolcano composed of five glacier-capped peaks along an 8 km-long NE-trending ridge. It is composed of five glacier-capped peaks along an 8 km-long NE-trending ridge. Several Holocene tephra layers have been documented from Yanteles volcano. Historical activity from this 2042 m high, andesitic volcanic complex is uncertain. Although there were reports of an eruption from Yanteles at the time of the 1835-02-20 Chile earthquake, and Sapper (1917) reported that previously unseen black areas were seen near the crater after the 1835 earthquake, the nature of this activity is not clear.</obo:IAO_0000115>
        <oboInOwl:hasOBONamespace>GAZ</oboInOwl:hasOBONamespace>
        <oboInOwl:id>GAZ:00056502</oboInOwl:id>
        <rdfs:label>Volcan Yanteles</rdfs:label>
    </owl:NamedIndividual>
    


    <!-- http://purl.obolibrary.org/obo/GAZ_00056504 -->

    <owl:NamedIndividual rdf:about="http://purl.obolibrary.org/obo/GAZ_00056504">
        <obo:RO_0001025 rdf:resource="http://purl.obolibrary.org/obo/GAZ_00136449"/>
        <obo:IAO_0000115>A chain of volcanoes in N Chile.</obo:IAO_0000115>
        <oboInOwl:hasOBONamespace>GAZ</oboInOwl:hasOBONamespace>
        <oboInOwl:id>GAZ:00056504</oboInOwl:id>
        <rdfs:label>Cordon de Puntas Negras</rdfs:label>
    </owl:NamedIndividual>
    


    <!-- http://purl.obolibrary.org/obo/GAZ_00056505 -->

    <owl:NamedIndividual rdf:about="http://purl.obolibrary.org/obo/GAZ_00056505">
        <obo:RO_0001025 rdf:resource="http://purl.obolibrary.org/obo/GAZ_00056504"/>
        <obo:IAO_0000115>A stratovolcano that is the common endpoint of two lines of volcanoes forming a V-shaped configuration. The northern chain is called Cordon de Puntas Negras, which terminates east of Chiliques volcano, and the southern chain is called Cordon Chalviri, whose southernmost summit is Cerro Tuyajto.</obo:IAO_0000115>
        <oboInOwl:hasOBONamespace>GAZ</oboInOwl:hasOBONamespace>
        <oboInOwl:id>GAZ:00056505</oboInOwl:id>
        <rdfs:label>Puntas Negras Volcano</rdfs:label>
    </owl:NamedIndividual>
    


    <!-- http://purl.obolibrary.org/obo/GAZ_00056506 -->

    <owl:NamedIndividual rdf:about="http://purl.obolibrary.org/obo/GAZ_00056506">
        <obo:RO_0001025 rdf:resource="http://purl.obolibrary.org/obo/GAZ_00136449"/>
        <oboInOwl:hasOBONamespace>GAZ</oboInOwl:hasOBONamespace>
        <oboInOwl:id>GAZ:00056506</oboInOwl:id>
        <rdfs:label>Cordon Chalviri</rdfs:label>
    </owl:NamedIndividual>
    


    <!-- http://purl.obolibrary.org/obo/GAZ_00056507 -->

    <owl:NamedIndividual rdf:about="http://purl.obolibrary.org/obo/GAZ_00056507">
        <obo:RO_0001025 rdf:resource="http://purl.obolibrary.org/obo/GAZ_00056506"/>
        <obo:IAO_0000115>The S point of the Cordon Chalviri.</obo:IAO_0000115>
        <oboInOwl:hasOBONamespace>GAZ</oboInOwl:hasOBONamespace>
        <oboInOwl:id>GAZ:00056507</oboInOwl:id>
        <rdfs:label>Cerro Tuyajto</rdfs:label>
    </owl:NamedIndividual>
    


    <!-- http://purl.obolibrary.org/obo/GAZ_00056508 -->

    <owl:NamedIndividual rdf:about="http://purl.obolibrary.org/obo/GAZ_00056508">
        <obo:RO_0001025 rdf:resource="http://purl.obolibrary.org/obo/GAZ_00136449"/>
        <obo:IAO_0000115>A small, inactive volcanic complex located on the Central Andes, at the border of Argentina and Chile. An older andesitic-dacitic edifice with a 1.3 km wide crater was mostly covered by younger Holocene andesitic lava flows. The youngest cone, 300 m high Volcan la Moyra, was the source of fresh-looking blocky andesitic lava flows that descended 6 km into Chile and 3 km into Argentina.</obo:IAO_0000115>
        <oboInOwl:hasOBONamespace>GAZ</oboInOwl:hasOBONamespace>
        <oboInOwl:id>GAZ:00056508</oboInOwl:id>
        <rdfs:label>Cordon del Azufre</rdfs:label>
    </owl:NamedIndividual>
    


    <!-- http://purl.obolibrary.org/obo/GAZ_00056509 -->

    <owl:NamedIndividual rdf:about="http://purl.obolibrary.org/obo/GAZ_00056509">
        <obo:RO_0001025 rdf:resource="http://purl.obolibrary.org/obo/GAZ_00136453"/>
        <obo:IAO_0000115>A stratovolcano located in the Maule Region of central Chile. It is a late-Pleistocene to Holocene andesitic-to-rhyodacitic stratovolcano with a 1.4 km wide ice-filled summit crater. Along with 3788 m high Cerro Azul, only 7 km to the south, 3953 m high Descabezado Grande lies at the center of a 20 x 30 km volcanic field. A lateral crater that formed on the upper NNE flank in 1932, shortly after the end of the major 1932 eruption from nearby Quizapu volcano on the north flank of Cerro Azul, was the site of the only historical eruption of Descabezado Grande. The Holocene Alto de las Mulas fissure on the lower NW flank of Descabezado Grande produced young rhyodacitic lava flows. Numerous small late-Pleistocene to Holocene volcanic centers are located north of the volcano. The northernmost of these, Lengua de Vulcano (or Mondaca) produced a very youthful rhyodacitic lava flow that dammed the Rio Lentue.</obo:IAO_0000115>
        <oboInOwl:hasOBONamespace>GAZ</oboInOwl:hasOBONamespace>
        <oboInOwl:id>GAZ:00056509</oboInOwl:id>
        <rdfs:label>Descabezado Grande</rdfs:label>
    </owl:NamedIndividual>
    


    <!-- http://purl.obolibrary.org/obo/GAZ_00056510 -->

    <owl:NamedIndividual rdf:about="http://purl.obolibrary.org/obo/GAZ_00056510">
        <obo:RO_0001025 rdf:resource="http://purl.obolibrary.org/obo/GAZ_00136449"/>
        <obo:IAO_0000115>A volcanic complex is a 15 km-long, E-W trending group of overlapping craters, lava domes, and composite cones extending from Chile into Argentina. The western portion includes the high point and principal edifice of the complex, Cerro Falso Azufre, and consists of overlapping craters that produced dominantly pyroclastic products. The eastern portion, located wholly in Argentina, contains two small composite cones and two lava domes that appear to represent the most recent activity of the complex (de Silva and Francis, 1991).</obo:IAO_0000115>
        <oboInOwl:hasOBONamespace>GAZ</oboInOwl:hasOBONamespace>
        <oboInOwl:id>GAZ:00056510</oboInOwl:id>
        <rdfs:label>Volcan Falso Azufre</rdfs:label>
    </owl:NamedIndividual>
    


    <!-- http://purl.obolibrary.org/obo/GAZ_00056511 -->

    <owl:NamedIndividual rdf:about="http://purl.obolibrary.org/obo/GAZ_00056511">
        <obo:RO_0001025 rdf:resource="http://purl.obolibrary.org/obo/GAZ_00056399"/>
        <obo:IAO_0000115>An active stratovolcano that lies just West of the border with Bolivia and at the South West end of the Nevados de Quimsachata. It is a symmetrical ice-clad stratovolcano at the SW end of the Nevados de Quimsachata volcano group. The 6071 m high Guallatiri lies just west of the border with Bolivia and is capped by a central dacitic dome or lava complex, with the active vent situated at its southern side. Thick lava flows are prominent on the lower northern and western flanks of the andesitic-to-rhyolitic volcano. Minor explosive eruptions have been reported from Guallatiri since the beginning of the 19th century. Intense fumarolic activity with &quot;jet-like&quot; noises continues, and numerous solfataras extend more than 300 m down the west flank.</obo:IAO_0000115>
        <oboInOwl:hasOBONamespace>GAZ</oboInOwl:hasOBONamespace>
        <oboInOwl:id>GAZ:00056511</oboInOwl:id>
        <rdfs:label>Volcan Guallatiri</rdfs:label>
    </owl:NamedIndividual>
    


    <!-- http://purl.obolibrary.org/obo/GAZ_00056512 -->

    <owl:NamedIndividual rdf:about="http://purl.obolibrary.org/obo/GAZ_00056512">
        <obo:RO_0001025 rdf:resource="http://purl.obolibrary.org/obo/GAZ_00056474"/>
        <obo:RO_0001025 rdf:resource="http://purl.obolibrary.org/obo/GAZ_00136453"/>
        <obo:IAO_0000115>A stratovolcano located in the Andes, in Los Lagos Region of Chile, south of the Yate Volcano. Located SSW of Volcan Yate, it is a morphologically youthful basaltic-andesite stratovolcano that is mostly forested. The 1572 m high volcano lies along a graben defined by the major regional Liquine-Ofqui fault zone, north of the Hornopiren strait and immediately south of Lago Cabrera. Prominent lava flows descend beyond the SW base of the volcano and overlie the graben floor. The volcano was said to be in eruption in 1835, although no details are known.</obo:IAO_0000115>
        <oboInOwl:hasOBONamespace>GAZ</oboInOwl:hasOBONamespace>
        <oboInOwl:id>GAZ:00056512</oboInOwl:id>
        <rdfs:label>Volcan Hornopiren</rdfs:label>
    </owl:NamedIndividual>
    


    <!-- http://purl.obolibrary.org/obo/GAZ_00056513 -->

    <owl:NamedIndividual rdf:about="http://purl.obolibrary.org/obo/GAZ_00056513">
        <obo:RO_0001025 rdf:resource="http://purl.obolibrary.org/obo/GAZ_00056474"/>
        <obo:RO_0001025 rdf:resource="http://purl.obolibrary.org/obo/GAZ_00136453"/>
        <obo:IAO_0000115>A stratovolcano located in the Andes, in Los Lagos Region of Chile, south of the Reloncavi Estuary. It is a late-Pleistocene, glacially dissected basaltic-andesite stratovolcano with Holocene parasitic vents. One of these flank vents is labeled Volcan Yate on the Volcan Hornopiren 1:50,000 quadrangle map. Little is known of the geologic history of this isolated volcano, located NNE of Volcan Hornopiren, south of the Relancavi strait. The elongated volcano contains six eruptive centers localized along a NW-trending fissure about 7.5 km long. The most recent activity originated from basaltic-andesite pyroclastic cones on the NW and western flanks. No historical eruptions are known from Volcan Yate, although the fresh morphology of its satellitic cones suggests an historical age (Gonzalez-Ferran, 1995).</obo:IAO_0000115>
        <oboInOwl:hasOBONamespace>GAZ</oboInOwl:hasOBONamespace>
        <oboInOwl:id>GAZ:00056513</oboInOwl:id>
        <rdfs:label>Volcan Yate</rdfs:label>
    </owl:NamedIndividual>
    


    <!-- http://purl.obolibrary.org/obo/GAZ_00056516 -->

    <owl:NamedIndividual rdf:about="http://purl.obolibrary.org/obo/GAZ_00056516">
        <obo:RO_0001025 rdf:resource="http://purl.obolibrary.org/obo/GAZ_00056517"/>
        <obo:RO_0001025 rdf:resource="http://purl.obolibrary.org/obo/GAZ_00136449"/>
        <obo:IAO_0000115>A volcano is located in Colchane, 7 km west of the Chile/Bolivia border and at the west end of a group of volcanoes lined up in a east-west direction, which also includes the volcanoes Cabaray and Tata Sabaya. Isluga has an elongated summit area and lies within the borders of Volcan Isluga National Park.</obo:IAO_0000115>
        <oboInOwl:hasOBONamespace>GAZ</oboInOwl:hasOBONamespace>
        <oboInOwl:id>GAZ:00056516</oboInOwl:id>
        <rdfs:label>Volcan Isluga</rdfs:label>
    </owl:NamedIndividual>
    


    <!-- http://purl.obolibrary.org/obo/GAZ_00056517 -->

    <owl:NamedIndividual rdf:about="http://purl.obolibrary.org/obo/GAZ_00056517">
        <obo:IAO_0000115>A national park located in the Andes, in the Tarapaca Region of Chile, near Colchane and south of Lauca Biosphere Reserve.</obo:IAO_0000115>
        <oboInOwl:hasOBONamespace>GAZ</oboInOwl:hasOBONamespace>
        <oboInOwl:id>GAZ:00056517</oboInOwl:id>
        <rdfs:label>Parque Nacional Volcan Isluga</rdfs:label>
    </owl:NamedIndividual>
    


    <!-- http://purl.obolibrary.org/obo/GAZ_00056518 -->

    <owl:NamedIndividual rdf:about="http://purl.obolibrary.org/obo/GAZ_00056518">
        <obo:RO_0001025 rdf:resource="http://purl.obolibrary.org/obo/GAZ_00136449"/>
        <obo:IAO_0000115>A stratovolcano. The most active volcano of the northern Chilean Andes. It lies east of the Salar de Atacama and immediately west of Aguas Calientes volcano. Prominent lava flows descend its NW flanks. An older, higher stratovolcano 5 km to the east, Volcan Aguas Calientes, displays a well-developed summit crater and a probable Holocene lava flow near its summit (de Silva and Francis, 1991). Lascar consists of two major edifices; activity began at the eastern volcano and then shifted to the western cone. The largest eruption of Lascar took place about 26,500 years ago, and following the eruption of the Tumbres scoria flow about 9000 years ago, activity shifted back to the eastern edifice, where three overlapping craters were formed.</obo:IAO_0000115>
        <oboInOwl:hasOBONamespace>GAZ</oboInOwl:hasOBONamespace>
        <oboInOwl:id>GAZ:00056518</oboInOwl:id>
        <rdfs:label>Volcan Lascar</rdfs:label>
    </owl:NamedIndividual>
    


    <!-- http://purl.obolibrary.org/obo/GAZ_00056519 -->

    <owl:NamedIndividual rdf:about="http://purl.obolibrary.org/obo/GAZ_00056519">
        <obo:IAO_0000115>A national park of Argentina, located in the province of Neuquen.</obo:IAO_0000115>
        <oboInOwl:hasOBONamespace>GAZ</oboInOwl:hasOBONamespace>
        <oboInOwl:id>GAZ:00056519</oboInOwl:id>
        <rdfs:label>Parque Nacional Lanin</rdfs:label>
    </owl:NamedIndividual>
    


    <!-- http://purl.obolibrary.org/obo/GAZ_00056520 -->

    <owl:NamedIndividual rdf:about="http://purl.obolibrary.org/obo/GAZ_00056520">
        <obo:RO_0001025 rdf:resource="http://purl.obolibrary.org/obo/GAZ_00056519"/>
        <obo:IAO_0000115>A lake in Neuquen Province, Patagonian Argentina. This glacial lake is located in the Andean mountains in Lanin National Park some 60 km from San Martin de los Andes.</obo:IAO_0000115>
        <oboInOwl:hasOBONamespace>GAZ</oboInOwl:hasOBONamespace>
        <oboInOwl:id>GAZ:00056520</oboInOwl:id>
        <rdfs:label>Lago Huechulafquen</rdfs:label>
    </owl:NamedIndividual>
    


    <!-- http://purl.obolibrary.org/obo/GAZ_00056521 -->

    <owl:NamedIndividual rdf:about="http://purl.obolibrary.org/obo/GAZ_00056521">
        <obo:RO_0001025 rdf:resource="http://purl.obolibrary.org/obo/GAZ_00056519"/>
        <obo:IAO_0000115>A lake of glacial origin in the province of Neuquen, Argentina. It is enclosed in a mountain range of the Andes.</obo:IAO_0000115>
        <oboInOwl:hasOBONamespace>GAZ</oboInOwl:hasOBONamespace>
        <oboInOwl:id>GAZ:00056521</oboInOwl:id>
        <rdfs:label>Lago Lacar</rdfs:label>
    </owl:NamedIndividual>
    


    <!-- http://purl.obolibrary.org/obo/GAZ_00056522 -->

    <owl:NamedIndividual rdf:about="http://purl.obolibrary.org/obo/GAZ_00056522">
        <obo:RO_0001025 rdf:resource="http://purl.obolibrary.org/obo/GAZ_00056519"/>
        <obo:RO_0001025 rdf:resource="http://purl.obolibrary.org/obo/GAZ_00056523"/>
        <obo:RO_0001025 rdf:resource="http://purl.obolibrary.org/obo/GAZ_00136453"/>
        <obo:IAO_0000115>An ice-clad, cone-shaped stratovolcano on the border of Argentina and Chile. It forms part of two national parks: Lanin in Argentina and Villarrica in Chile. The dominantly effusive basaltic-to-trachydacitic volcano lies at the eastern end of a NW-SE-trending volcanic group beginning with Villarrica that is transverse to the Andean chain. The beautifully symmetrical, 3737 m high Lanin rises 2500 m above its base; shoulder areas on the upper flanks hint at a buried caldera. The volcano was formed in four eruptive stages dating back to the early Pleistocene or late Pliocene. The last two stages occurred during the late-Pleistocene and Holocene. A small lava dome at the summit fed blocky lava flows to the north about 2200 years ago. A postglacial tuff ring (Volcan Arenal) is located below the SW flank of Lanin in Argentina. A younger lava flow from Lanin covers deposits of Volcan Arenal and extends south into Lago Paimun.</obo:IAO_0000115>
        <oboInOwl:hasOBONamespace>GAZ</oboInOwl:hasOBONamespace>
        <oboInOwl:id>GAZ:00056522</oboInOwl:id>
        <rdfs:label>Volcan Lanin</rdfs:label>
    </owl:NamedIndividual>
    


    <!-- http://purl.obolibrary.org/obo/GAZ_00056523 -->

    <owl:NamedIndividual rdf:about="http://purl.obolibrary.org/obo/GAZ_00056523">
        <obo:IAO_0000115>A national park located in the Andes, in the Araucania Region of Chile, near Pucon. The centerpiece of the park is a line of three volcanoes stretching transversely to the Andean range: Villarrica, Quetrupillan and Lanin.</obo:IAO_0000115>
        <oboInOwl:hasOBONamespace>GAZ</oboInOwl:hasOBONamespace>
        <oboInOwl:id>GAZ:00056523</oboInOwl:id>
        <rdfs:label>Parque Nacional Villarrica</rdfs:label>
    </owl:NamedIndividual>
    


    <!-- http://purl.obolibrary.org/obo/GAZ_00056524 -->

    <owl:NamedIndividual rdf:about="http://purl.obolibrary.org/obo/GAZ_00056524">
        <obo:RO_0001025 rdf:resource="http://purl.obolibrary.org/obo/GAZ_00056523"/>
        <obo:RO_0001025 rdf:resource="http://purl.obolibrary.org/obo/GAZ_00136453"/>
        <obo:IAO_0000115>An active stratovolcano. It is the westernmost of three large stratovolcanoes that trend perpendicular to the Andean chain. A 6 km wide caldera formed during the late Pleistocene. A 2 km wide caldera that formed about 3500 years ago is located at the base of the presently active, dominantly basaltic to basaltic-andesitic cone at the NW margin of the Pleistocene caldera. More than 30 scoria cones and fissure vents dot Villarrica&apos;s flanks. Plinian eruptions and pyroclastic flows that have extended up to 20 km from the volcano have been produced during the Holocene. Lava flows up to 18 km long have issued from summit and flank vents. Historical eruptions, documented since 1558, have consisted largely of mild-to-moderate explosive activity with occasional lava effusion. Glaciers cover 40 km2 of the volcano, and lahars have damaged towns on its flanks.</obo:IAO_0000115>
        <oboInOwl:hasOBONamespace>GAZ</oboInOwl:hasOBONamespace>
        <oboInOwl:id>GAZ:00056524</oboInOwl:id>
        <rdfs:label>Volcan Villarrica</rdfs:label>
    </owl:NamedIndividual>
    


    <!-- http://purl.obolibrary.org/obo/GAZ_00056525 -->

    <owl:NamedIndividual rdf:about="http://purl.obolibrary.org/obo/GAZ_00056525">
        <obo:RO_0001025 rdf:resource="http://purl.obolibrary.org/obo/GAZ_00056523"/>
        <obo:RO_0001025 rdf:resource="http://purl.obolibrary.org/obo/GAZ_00136453"/>
        <obo:IAO_0000115>A stratovolcano located in the Araucania Region of Chile. It is situated between Villarrica and Lanin volcanoes, within Villarrica National Park. The late-Pleistocene to Holocene Quetrupillan stratovolcano is at the center of a group of three volcanoes trending transverse to the Andean chain. Constructed within a large 7 x 10 km wide caldera, 2360 m high, glacier-covered Quetrupillan contains a 3.5 km wide caldera and has more silicic lavas than its more prominent neighbors Villarrica and Lanin. The basaltic scoria cone Huililco lies 12 km NE of Quetrupillan, a rhyolitic lava dome lies on the south flank of the caldera, and the Volcanes de Reyehueico produced basaltic-andesite lava flows 15 km south of the summit caldera. Some of the most recent activity produced the Volcanes de Llancahue pyroclastic cones near the SW margin of the older caldera.</obo:IAO_0000115>
        <oboInOwl:hasOBONamespace>GAZ</oboInOwl:hasOBONamespace>
        <oboInOwl:id>GAZ:00056525</oboInOwl:id>
        <rdfs:label>Volcan Quetrupillan</rdfs:label>
    </owl:NamedIndividual>
    


    <!-- http://purl.obolibrary.org/obo/GAZ_00056526 -->

    <owl:NamedIndividual rdf:about="http://purl.obolibrary.org/obo/GAZ_00056526">
        <obo:RO_0001025 rdf:resource="http://purl.obolibrary.org/obo/GAZ_00136449"/>
        <obo:IAO_0000115>A stratovolcano along the border of Argentina and Chile. It contains five nested summit craters. The youngest feature is a lava dome that overlaps the northern crater rim. The large andesitic-dacitic Negriales lava field on the western flanks was erupted from a single SW-flank vent. A large debris-avalanche deposit is found on the SE flank. Recent pyroclastic-flow deposits form an extensive apron below the northern flanks of the volcano. Although no historical eruptions have been recorded, the youthful morphology of deposits suggest that Lastarria has been active during historical time. Persistent fumarolic activity occurs at the summit and NW flank, and sulfur flows have been produced by melting of extensive sulfur deposits in the summit region.</obo:IAO_0000115>
        <oboInOwl:hasOBONamespace>GAZ</oboInOwl:hasOBONamespace>
        <oboInOwl:id>GAZ:00056526</oboInOwl:id>
        <rdfs:label>Volcan Lastarria</rdfs:label>
    </owl:NamedIndividual>
    


    <!-- http://purl.obolibrary.org/obo/GAZ_00056534 -->

    <owl:NamedIndividual rdf:about="http://purl.obolibrary.org/obo/GAZ_00056534">
        <obo:RO_0001025 rdf:resource="http://purl.obolibrary.org/obo/GAZ_00136454"/>
        <obo:IAO_0000115>An active ice-covered volcano located in Chilean Patagonia, in the northern part of the Southern Patagonian Ice Field. Glacier-covered, 3607 m high Lautaro volcano, the highest Chilean volcano below 40 degrees south, rises above the Southern Patagonian Ice Field. It has a crater just below its summit on the NW side, and a 1 km wide crater is located on the NE flank. Ash deposits from eruptions of this dominantly dacitic volcano were visible on aerial photos taken during several occasions during the 20th century, and older ash layers form prominent markers on outflow glaciers of the Patagonian icecap.</obo:IAO_0000115>
        <oboInOwl:hasOBONamespace>GAZ</oboInOwl:hasOBONamespace>
        <oboInOwl:id>GAZ:00056534</oboInOwl:id>
        <rdfs:label>Volcan Lautaro</rdfs:label>
    </owl:NamedIndividual>
    


    <!-- http://purl.obolibrary.org/obo/GAZ_00056535 -->

    <owl:NamedIndividual rdf:about="http://purl.obolibrary.org/obo/GAZ_00056535">
        <obo:RO_0001025 rdf:resource="http://purl.obolibrary.org/obo/GAZ_00120477"/>
        <obo:IAO_0000115>A shallow saline lake in the southwest of the altiplano of Bolivia, within Eduardo Avaroa Andean Fauna National Reserve and close to the border with Chile. The lake contains borax islands. A Ramsar Site.</obo:IAO_0000115>
        <oboInOwl:hasOBONamespace>GAZ</oboInOwl:hasOBONamespace>
        <oboInOwl:id>GAZ:00056535</oboInOwl:id>
        <rdfs:label>Laguna Colorada</rdfs:label>
    </owl:NamedIndividual>
    


    <!-- http://purl.obolibrary.org/obo/GAZ_00056536 -->

    <owl:NamedIndividual rdf:about="http://purl.obolibrary.org/obo/GAZ_00056536">
        <obo:RO_0001025 rdf:resource="http://purl.obolibrary.org/obo/GAZ_00136449"/>
        <obo:IAO_0000115>A stratovolcano on the border between Bolivia and Chile. In its vicinity lie Laguna Colorada and Cerro del Leon.</obo:IAO_0000115>
        <oboInOwl:hasOBONamespace>GAZ</oboInOwl:hasOBONamespace>
        <oboInOwl:id>GAZ:00056536</oboInOwl:id>
        <rdfs:label>Volcan Linzor</rdfs:label>
    </owl:NamedIndividual>
    


    <!-- http://purl.obolibrary.org/obo/GAZ_00056538 -->

    <owl:NamedIndividual rdf:about="http://purl.obolibrary.org/obo/GAZ_00056538">
        <obo:IAO_0000115>A national park located in the Andes, in the provinces of Cautin and Malleco, in the Araucania Region of Chile. Established 1940.</obo:IAO_0000115>
        <oboInOwl:hasOBONamespace>GAZ</oboInOwl:hasOBONamespace>
        <oboInOwl:id>GAZ:00056538</oboInOwl:id>
        <rdfs:label>Parque Nacional Conguillio</rdfs:label>
    </owl:NamedIndividual>
    


    <!-- http://purl.obolibrary.org/obo/GAZ_00056539 -->

    <owl:NamedIndividual rdf:about="http://purl.obolibrary.org/obo/GAZ_00056539">
        <obo:RO_0001025 rdf:resource="http://purl.obolibrary.org/obo/GAZ_00056538"/>
        <obo:RO_0001025 rdf:resource="http://purl.obolibrary.org/obo/GAZ_00136453"/>
        <obo:IAO_0000115>A stratovolcano located 82 km northeast of Temuco and 663 km southeast of Santiago, within the borders of Conguillio National Park. The massive 3125 m high, dominantly basaltic-to-andesitic stratovolcano has a volume of 400 cu km. A Holocene edifice built primarily of accumulated lava flows was constructed over an 8 km wide caldera that formed about 13,200 years ago, following the eruption of the 24 cu km Curacautin Ignimbrite. More than 40 scoria cones dot the volcano&apos;s flanks. Following the end of an explosive stage about 7200 years ago, construction of the present edifice began, characterized by strombolian, hawaiian, and infrequent subplinian eruptions. Frequent moderate explosive eruptions with occasional lava flows have been recorded since the 17th century.</obo:IAO_0000115>
        <oboInOwl:hasOBONamespace>GAZ</oboInOwl:hasOBONamespace>
        <oboInOwl:id>GAZ:00056539</oboInOwl:id>
        <rdfs:label>Volcan Llaima Volcano</rdfs:label>
    </owl:NamedIndividual>
    


    <!-- http://purl.obolibrary.org/obo/GAZ_00056540 -->

    <owl:NamedIndividual rdf:about="http://purl.obolibrary.org/obo/GAZ_00056540">
        <obo:RO_0001025 rdf:resource="http://purl.obolibrary.org/obo/GAZ_00056538"/>
        <obo:IAO_0000115>A freshwater lake located in the Araucania Region of Chile, within the Conguillio National Park.</obo:IAO_0000115>
        <oboInOwl:hasOBONamespace>GAZ</oboInOwl:hasOBONamespace>
        <oboInOwl:id>GAZ:00056540</oboInOwl:id>
        <rdfs:label>Lago Conguillio</rdfs:label>
    </owl:NamedIndividual>
    


    <!-- http://purl.obolibrary.org/obo/GAZ_00056541 -->

    <owl:NamedIndividual rdf:about="http://purl.obolibrary.org/obo/GAZ_00056541">
        <obo:RO_0001025 rdf:resource="http://purl.obolibrary.org/obo/GAZ_00136449"/>
        <obo:IAO_0000115>A region of very high volcanic peaks on a high plateau within the Atacama Desert. Extends from Chile to Argentina.</obo:IAO_0000115>
        <oboInOwl:hasOBONamespace>GAZ</oboInOwl:hasOBONamespace>
        <oboInOwl:id>GAZ:00056541</oboInOwl:id>
        <rdfs:label>Puna de Atacama</rdfs:label>
    </owl:NamedIndividual>
    


    <!-- http://purl.obolibrary.org/obo/GAZ_00056542 -->

    <owl:NamedIndividual rdf:about="http://purl.obolibrary.org/obo/GAZ_00056542">
        <obo:RO_0001025 rdf:resource="http://purl.obolibrary.org/obo/GAZ_00056541"/>
        <obo:RO_0001025 rdf:resource="http://purl.obolibrary.org/obo/GAZ_00136449"/>
        <obo:IAO_0000115>A stratovolcano at the border of Argentina (Salta Province) and Chile. It lies in the Puna de Atacama, a region of very high volcanic peaks on a high plateau within the Atacama Desert. The summit is formed by a smaller well-preserved cone that was constructed on an older Pleistocene edifice. A major debris-avalanche deposit produced by collapse of the older volcano about 150,000 years ago extends eastward into Argentina and diverges around the north and south sides of the older Cerro Rosado stratovolcano 17 km east of Llullaillaco. Construction of several lava domes and flows was associated with growth of the modern cone. The two most prominent flows contain distinct flow levees and ridges and extend down the northern and southern flanks. These two extremely youthful-looking dacitic flows were initially considered to be of Holocene age, but more recent Ar/Ar dating indicates that they are of late Pleistocene age (Richards and Villeneuve, 2001).</obo:IAO_0000115>
        <oboInOwl:hasOBONamespace>GAZ</oboInOwl:hasOBONamespace>
        <oboInOwl:id>GAZ:00056542</oboInOwl:id>
        <rdfs:label>Volcan Llullaillaco</rdfs:label>
    </owl:NamedIndividual>
    


    <!-- http://purl.obolibrary.org/obo/GAZ_00056544 -->

    <owl:NamedIndividual rdf:about="http://purl.obolibrary.org/obo/GAZ_00056544">
        <obo:RO_0001025 rdf:resource="http://purl.obolibrary.org/obo/GAZ_00056545"/>
        <obo:RO_0001025 rdf:resource="http://purl.obolibrary.org/obo/GAZ_00136453"/>
        <obo:IAO_0000115>A stratovolcano of late-Pleistocene to dominantly Holocene age, with the shape of a truncated cone. It is located in the Araucania Region of Chile, immediately SE of Tolhuaca volcano. A glacier fills its summit crater and spills down the south flank. The volcano is dominantly andesitic, but basaltic and dacitic rocks are also present. An E-W-trending fissure is present, but a prominent NE-SW fissure cuts across the entire volcano. The Cordon Fissural Oriental fissure zone extends 10 km to the NE and has produced a series of NE-flank vents and cinder cones, some of which have been the source of voluminous lava flows in historical time. Major lava flows erupted during 1887-90 and 1988-90 traveled up to 10 km from their NE-flank vents.</obo:IAO_0000115>
        <oboInOwl:hasOBONamespace>GAZ</oboInOwl:hasOBONamespace>
        <oboInOwl:id>GAZ:00056544</oboInOwl:id>
        <rdfs:label>Volcan Lonquimay</rdfs:label>
    </owl:NamedIndividual>
    


    <!-- http://purl.obolibrary.org/obo/GAZ_00056545 -->

    <owl:NamedIndividual rdf:about="http://purl.obolibrary.org/obo/GAZ_00056545">
        <obo:IAO_0000115>A protected area comprising two adjoining national reserves: Malalcahuello and Nalcas. It is located in the Andes, in the Araucania Region of Chile and bordering the Bio-Bio Region.</obo:IAO_0000115>
        <oboInOwl:hasOBONamespace>GAZ</oboInOwl:hasOBONamespace>
        <oboInOwl:id>GAZ:00056545</oboInOwl:id>
        <rdfs:label>Malalcahuello-Nalcas</rdfs:label>
    </owl:NamedIndividual>
    


    <!-- http://purl.obolibrary.org/obo/GAZ_00056546 -->

    <owl:NamedIndividual rdf:about="http://purl.obolibrary.org/obo/GAZ_00056546">
        <obo:RO_0001025 rdf:resource="http://purl.obolibrary.org/obo/GAZ_00056545"/>
        <obo:RO_0001025 rdf:resource="http://purl.obolibrary.org/obo/GAZ_00056548"/>
        <obo:RO_0001025 rdf:resource="http://purl.obolibrary.org/obo/GAZ_00136453"/>
        <obo:IAO_0000115>A stratovolcano located in the northern part of the Araucania Region of Chile.</obo:IAO_0000115>
        <oboInOwl:hasOBONamespace>GAZ</oboInOwl:hasOBONamespace>
        <oboInOwl:id>GAZ:00056546</oboInOwl:id>
        <rdfs:label>Volcan Tolhuaca</rdfs:label>
    </owl:NamedIndividual>
    


    <!-- http://purl.obolibrary.org/obo/GAZ_00056547 -->

    <owl:NamedIndividual rdf:about="http://purl.obolibrary.org/obo/GAZ_00056547">
        <obo:RO_0001025 rdf:resource="http://purl.obolibrary.org/obo/GAZ_00056538"/>
        <obo:RO_0001025 rdf:resource="http://purl.obolibrary.org/obo/GAZ_00136453"/>
        <obo:IAO_0000115>A stratovolcano located in the Araucania Region of Chile, near the Llaima volcano.</obo:IAO_0000115>
        <oboInOwl:hasOBONamespace>GAZ</oboInOwl:hasOBONamespace>
        <oboInOwl:id>GAZ:00056547</oboInOwl:id>
        <rdfs:label>Volcan Sierra Nevada Volcano</rdfs:label>
    </owl:NamedIndividual>
    


    <!-- http://purl.obolibrary.org/obo/GAZ_00056548 -->

    <owl:NamedIndividual rdf:about="http://purl.obolibrary.org/obo/GAZ_00056548">
        <obo:IAO_0000115>A national park located on the western slope of the Andes, in the Araucania Region of Chile. It has an elevation of 700 m asl at its western end and 1,821 m asl at its eastern end. The Malleco River&apos;s source is located within the park.</obo:IAO_0000115>
        <oboInOwl:hasOBONamespace>GAZ</oboInOwl:hasOBONamespace>
        <oboInOwl:id>GAZ:00056548</oboInOwl:id>
        <rdfs:label>Parque Nacional Tolhuaca</rdfs:label>
    </owl:NamedIndividual>
    


    <!-- http://purl.obolibrary.org/obo/GAZ_00056549 -->

    <owl:NamedIndividual rdf:about="http://purl.obolibrary.org/obo/GAZ_00056549">
        <obo:RO_0001025 rdf:resource="http://purl.obolibrary.org/obo/GAZ_00136453"/>
        <obo:IAO_0000115>A stratovolcano located to the north of the Aysen Fjord and to the east of the Moraleda Channel, in the Aysen Region of Chile. This glacier-covered, basaltic-to-dacitic stratovolcano lies within a caldera and contains a summit lava dome. Five flank cinder cones and lava domes lie along a NE-trending fissure that extends 15 km from the summit. The volcano lies along the regional Liquine-Ofqui fault zone, and tephra layer of late-Holocene age was documented.</obo:IAO_0000115>
        <oboInOwl:hasOBONamespace>GAZ</oboInOwl:hasOBONamespace>
        <oboInOwl:id>GAZ:00056549</oboInOwl:id>
        <rdfs:label>Volcan Maca</rdfs:label>
    </owl:NamedIndividual>
    


    <!-- http://purl.obolibrary.org/obo/GAZ_00056550 -->

    <owl:NamedIndividual rdf:about="http://purl.obolibrary.org/obo/GAZ_00056550">
        <obo:RO_0001025 rdf:resource="http://purl.obolibrary.org/obo/GAZ_00136453"/>
        <obo:IAO_0000115>A stratovolcano with an 8 km wide, largely buried caldera located about 40 km NW of the town of Puerto Puyuhuapi, in the Aysen Region of Chile. It lies near of the entrance of the Moraleda Channel.</obo:IAO_0000115>
        <oboInOwl:hasOBONamespace>GAZ</oboInOwl:hasOBONamespace>
        <oboInOwl:id>GAZ:00056550</oboInOwl:id>
        <rdfs:label>Volcan Melimoyu</rdfs:label>
    </owl:NamedIndividual>
    


    <!-- http://purl.obolibrary.org/obo/GAZ_00056551 -->

    <owl:NamedIndividual rdf:about="http://purl.obolibrary.org/obo/GAZ_00056551">
        <obo:RO_0001025 rdf:resource="http://purl.obolibrary.org/obo/GAZ_00136453"/>
        <obo:IAO_0000115>An ice-filled 6 km wide caldera in the central portion of Magdalena Island. It forms part of the Isla Magdalena National Park. An eruption about 7000 years ago produced a pumice and scoria layer that extends to the SE. A young-looking andesitic lava flow on the west side of the volcano may be its most recent product. Historical reports by Serrano describe an eruption at the beginning of the 18th century that could refer to this lava flow.</obo:IAO_0000115>
        <oboInOwl:hasOBONamespace>GAZ</oboInOwl:hasOBONamespace>
        <oboInOwl:id>GAZ:00056551</oboInOwl:id>
        <rdfs:label>Volcan Mentolat</rdfs:label>
    </owl:NamedIndividual>
    


    <!-- http://purl.obolibrary.org/obo/GAZ_00056554 -->

    <owl:NamedIndividual rdf:about="http://purl.obolibrary.org/obo/GAZ_00056554">
        <obo:RO_0001025 rdf:resource="http://purl.obolibrary.org/obo/GAZ_00136453"/>
        <oboInOwl:hasOBONamespace>GAZ</oboInOwl:hasOBONamespace>
        <oboInOwl:id>GAZ:00056554</oboInOwl:id>
        <rdfs:label>Diamante Caldera</rdfs:label>
    </owl:NamedIndividual>
    


    <!-- http://purl.obolibrary.org/obo/GAZ_00056555 -->

    <owl:NamedIndividual rdf:about="http://purl.obolibrary.org/obo/GAZ_00056555">
        <obo:RO_0001025 rdf:resource="http://purl.obolibrary.org/obo/GAZ_00056554"/>
        <obo:RO_0001025 rdf:resource="http://purl.obolibrary.org/obo/GAZ_00136453"/>
        <obo:IAO_0000115>A stratovolcano in the Andes, lying on the border between Argentina and Chile. It is located 90 km south of Tupungato and about 100 km SE of Santiago. Maipo is located within the Diamante Caldera, a feature of about 15 km by 20 km size that is about one-half million years old.</obo:IAO_0000115>
        <oboInOwl:hasOBONamespace>GAZ</oboInOwl:hasOBONamespace>
        <oboInOwl:id>GAZ:00056555</oboInOwl:id>
        <rdfs:label>Volcan Maipo</rdfs:label>
    </owl:NamedIndividual>
    


    <!-- http://purl.obolibrary.org/obo/GAZ_00056556 -->

    <owl:NamedIndividual rdf:about="http://purl.obolibrary.org/obo/GAZ_00056556">
        <obo:RO_0001025 rdf:resource="http://purl.obolibrary.org/obo/GAZ_00056554"/>
        <obo:IAO_0000115>A freshwater lake located in the province of Mendoza, Argentina, in the San Carlos Department, some 198 km from Mendoza.</obo:IAO_0000115>
        <oboInOwl:hasOBONamespace>GAZ</oboInOwl:hasOBONamespace>
        <oboInOwl:id>GAZ:00056556</oboInOwl:id>
        <rdfs:label>Laguna del Diamante</rdfs:label>
    </owl:NamedIndividual>
    


    <!-- http://purl.obolibrary.org/obo/GAZ_00056558 -->

    <owl:NamedIndividual rdf:about="http://purl.obolibrary.org/obo/GAZ_00056558">
        <obo:RO_0001025 rdf:resource="http://purl.obolibrary.org/obo/GAZ_00136453"/>
        <obo:IAO_0000115>A stratovolcano located in Los Lagos Region of Chile. It is west of Lago Renihue, has a saddle-shaped summit with an elongated 3 km wide caldera. The massive edifice is elongated in a NE-SW direction, and a youthful eruptive center is located on the ENE side of the complex. Two major explosive eruptions during the Holocene produced tephra deposits extending to the east. An eruption from Minchinmavida was reported in 1742. Darwin observed the volcano in activity in 1834 on his renowned voyage that took him to the Galapagos Islands. The latest known eruption of basaltic-to-andesitic Minchinmavida, from 1835-02 to 1835-03, produced a lava flow from a flank crater and lahars that reached the coast at Punta Chana.</obo:IAO_0000115>
        <oboInOwl:hasOBONamespace>GAZ</oboInOwl:hasOBONamespace>
        <oboInOwl:id>GAZ:00056558</oboInOwl:id>
        <rdfs:label>Volcan Michinmahuida</rdfs:label>
    </owl:NamedIndividual>
    


    <!-- http://purl.obolibrary.org/obo/GAZ_00056559 -->

    <owl:NamedIndividual rdf:about="http://purl.obolibrary.org/obo/GAZ_00056559">
        <rdf:type rdf:resource="http://purl.obolibrary.org/obo/ENVO_00000354"/>
        <obo:RO_0001025 rdf:resource="http://purl.obolibrary.org/obo/GAZ_00136449"/>
        <obo:IAO_0000115>A volcanic complex located in the Antofagasta Region of Chile, south of Laguna Miscanti.</obo:IAO_0000115>
        <oboInOwl:hasOBONamespace>GAZ</oboInOwl:hasOBONamespace>
        <oboInOwl:id>GAZ:00056559</oboInOwl:id>
        <rdfs:label>Miniques Volcanic Complex</rdfs:label>
    </owl:NamedIndividual>
    


    <!-- http://purl.obolibrary.org/obo/GAZ_00056560 -->

    <owl:NamedIndividual rdf:about="http://purl.obolibrary.org/obo/GAZ_00056560">
        <obo:RO_0001025 rdf:resource="http://purl.obolibrary.org/obo/GAZ_00136449"/>
        <obo:IAO_0000115>A mountain located in the Antofagasta Region of Chile, immediately south of Chiliques and north of Miniques. It towers over Laguna Miscanti.</obo:IAO_0000115>
        <oboInOwl:hasOBONamespace>GAZ</oboInOwl:hasOBONamespace>
        <oboInOwl:id>GAZ:00056560</oboInOwl:id>
        <rdfs:label>Cerro Miscanti</rdfs:label>
    </owl:NamedIndividual>
    


    <!-- http://purl.obolibrary.org/obo/GAZ_00056561 -->

    <owl:NamedIndividual rdf:about="http://purl.obolibrary.org/obo/GAZ_00056561">
        <obo:RO_0001025 rdf:resource="http://purl.obolibrary.org/obo/GAZ_00136449"/>
        <obo:IAO_0000115>A mountain with several summits located in the Antofagasta Region of Chile, near Sico Pass.</obo:IAO_0000115>
        <oboInOwl:hasOBONamespace>GAZ</oboInOwl:hasOBONamespace>
        <oboInOwl:id>GAZ:00056561</oboInOwl:id>
        <rdfs:label>Cerros de Incahuasi</rdfs:label>
    </owl:NamedIndividual>
    


    <!-- http://purl.obolibrary.org/obo/GAZ_00056563 -->

    <owl:NamedIndividual rdf:about="http://purl.obolibrary.org/obo/GAZ_00056563">
        <obo:RO_0001025 rdf:resource="http://purl.obolibrary.org/obo/GAZ_00056564"/>
        <obo:RO_0001025 rdf:resource="http://purl.obolibrary.org/obo/GAZ_00136453"/>
        <obo:IAO_0000115>A stratovolcano in the Chilean province of Valdivia in the Andes. The compound Mocho-Choshuenco volcano is composed of twin glacier-covered stratovolcanoes, located east of Lago Rinihue and SE of Lago Panguipulli and post-dating a 4 km wide basaltic caldera. The small 2415 m high Choshuenco stratovolcano, constructed on the NW rim of the caldera, is late-glacial in age. A major plinian eruption produced the Neltume Pumice about 10,300 years ago. The larger andesitic-to-dacitic, 2422 m high El Mocho volcano, constructed within the caldera, is postglacial and has been historically active. Parasitic craters and basaltic scoria cones are located on the flanks of Mocho-Choshuenco, primarily on the NE and SW sides. Two historical eruptions have been reported, one in 1864 and the other in 1937.</obo:IAO_0000115>
        <oboInOwl:hasOBONamespace>GAZ</oboInOwl:hasOBONamespace>
        <oboInOwl:id>GAZ:00056563</oboInOwl:id>
        <rdfs:label>Volcan Mocho-Choshuenco</rdfs:label>
    </owl:NamedIndividual>
    


    <!-- http://purl.obolibrary.org/obo/GAZ_00056564 -->

    <owl:NamedIndividual rdf:about="http://purl.obolibrary.org/obo/GAZ_00056564">
        <obo:IAO_0000115>A protected area around the Mocho-Choshuenco volcano, in Valdivia Province, southern Chile.</obo:IAO_0000115>
        <oboInOwl:hasOBONamespace>GAZ</oboInOwl:hasOBONamespace>
        <oboInOwl:id>GAZ:00056564</oboInOwl:id>
        <rdfs:label>Reserva Nacional Mocho-Choshuenco</rdfs:label>
    </owl:NamedIndividual>
    


    <!-- http://purl.obolibrary.org/obo/GAZ_00056583 -->

    <owl:NamedIndividual rdf:about="http://purl.obolibrary.org/obo/GAZ_00056583">
        <obo:RO_0001025 rdf:resource="http://purl.obolibrary.org/obo/GAZ_00136454"/>
        <obo:IAO_0000115>A volcano located in the Patagonian region of Chile, on Peninsula Munoz Gamero and south of Cordillera Sarmiento. This ice-covered volcano lies about 200 km North-West of the city of Punta Arenas. Monte Burney was constructed on the western rim of a 6 km wide caldera, which is partially filled with and surrounded by an unglaciated pyroclastic-flow deposit. Flank vents produced andesitic-dacitic lava flows and pyroclastic material. Collapse of the edifice produced a major debris avalanche that traveled to the SSW. Two large plinian eruptions have been documented from Monte Burney during the Holocene. The only known historical eruption of Monte Burney took place in 1910.</obo:IAO_0000115>
        <oboInOwl:hasOBONamespace>GAZ</oboInOwl:hasOBONamespace>
        <oboInOwl:id>GAZ:00056583</oboInOwl:id>
        <rdfs:label>Monte Burney</rdfs:label>
    </owl:NamedIndividual>
    


    <!-- http://purl.obolibrary.org/obo/GAZ_00056588 -->

    <owl:NamedIndividual rdf:about="http://purl.obolibrary.org/obo/GAZ_00056588">
        <obo:IAO_0000115>A short mountain range mantled by an ice field. It is located in the southwestern portion of Isla Grande de Tierra del Fuego, entirely within the Chilean territory. It is part of the longest Andes range.</obo:IAO_0000115>
        <oboInOwl:hasOBONamespace>GAZ</oboInOwl:hasOBONamespace>
        <oboInOwl:id>GAZ:00056588</oboInOwl:id>
        <rdfs:label>Cordillera Darwin</rdfs:label>
    </owl:NamedIndividual>
    


    <!-- http://purl.obolibrary.org/obo/GAZ_00056594 -->

    <owl:NamedIndividual rdf:about="http://purl.obolibrary.org/obo/GAZ_00056594">
        <obo:RO_0001025 rdf:resource="http://purl.obolibrary.org/obo/GAZ_00136449"/>
        <obo:IAO_0000115>A complex volcanic massif that straddles the Chile-Argentina border ENE of Nevados Ojos del Salado volcano. Two stratovolcanoes occupy a compound 3.5 km wide caldera, and Pleistocene lava domes are located on the west and SW flanks of the 6621 m high volcano. The youngest stratovolcano is capped by a 1 km wide crater, and dacitic lava flows radiate down the volcano&apos;s flanks. The fresh-looking morphology of the youngest products of Nevado de Incahuasi suggest a Holocene age (Gonzalez-Ferran, 1995). A dacitic lava dome partially fills an arcuate crater on the eastern flank of Incahuasi. Four pyroclastic cones are located 7 km to NE and produced basaltic-andesite lava flows that cover an area of 10 sq km.</obo:IAO_0000115>
        <oboInOwl:hasOBONamespace>GAZ</oboInOwl:hasOBONamespace>
        <oboInOwl:id>GAZ:00056594</oboInOwl:id>
        <rdfs:label>Nevado de Incahuasi</rdfs:label>
    </owl:NamedIndividual>
    


    <!-- http://purl.obolibrary.org/obo/GAZ_00056595 -->

    <owl:NamedIndividual rdf:about="http://purl.obolibrary.org/obo/GAZ_00056595">
        <obo:RO_0001025 rdf:resource="http://purl.obolibrary.org/obo/GAZ_00136453"/>
        <obo:IAO_0000115>A stratovolcano in the Andes of central Chile. The 3,242 m perennially snowcapped peak is a landmark of Linares Province and the Maule Region. It is a late-Pleistocene to Holocene, dominantly andesitic stratovolcano constructed over a basement of Tertiary volcaniclastic and granitic rocks. Two edifice-collapse events modified the eastern and SW flank of a pre-Holocene volcano, and Holocene activity has been concentrated at the summit region and on the eastern flanks of the volcano. Andesitic-to-dacitic lava domes occupy the summit region, and a Holocene dome forms the 3242 m high summit of Longavi. The last eruptions produced a lava dome in the upper part of the collapse scarp and summit region that partially collapsed to the east, forming block-and-ash flow deposits. No historical eruptions are known, although fumarolic activity continues.</obo:IAO_0000115>
        <oboInOwl:hasOBONamespace>GAZ</oboInOwl:hasOBONamespace>
        <oboInOwl:id>GAZ:00056595</oboInOwl:id>
        <rdfs:label>Nevado de Longavi</rdfs:label>
    </owl:NamedIndividual>
    


    <!-- http://purl.obolibrary.org/obo/GAZ_00056596 -->

    <owl:NamedIndividual rdf:about="http://purl.obolibrary.org/obo/GAZ_00056596">
        <obo:RO_0001025 rdf:resource="http://purl.obolibrary.org/obo/GAZ_00136453"/>
        <obo:IAO_0000115>A group of stratovolcanoes located in the Andes of the Bio-Bio Region, Chile. Three late-Pleistocene to Holocene stratovolcanoes were constructed along a NNW-SSE line within three nested Pleistocene calderas, which produced ignimbrite sheets extending more than 100 km into the Central Depression of Chile. The largest stratovolcano, dominantly andesitic, 3212 m high Volcan Nevado, is located at the NW end of the group, and 3089 m high Volcan Viejo, which was the main active vent during the 17th-19th centuries, occupies the SE end. The new Volcan Nuevo lava-dome complex formed between 1906 and 1945 between the two volcanoes and grew to exceed Volcan Viejo in altitude. The Volcan Arrau dome complex was constructed SE of Volcan Nuevo between 1973 and 1986, eventually exceeding its height by 20 m.</obo:IAO_0000115>
        <oboInOwl:hasOBONamespace>GAZ</oboInOwl:hasOBONamespace>
        <oboInOwl:id>GAZ:00056596</oboInOwl:id>
        <rdfs:label>Nevados de Chillan</rdfs:label>
    </owl:NamedIndividual>
    


    <!-- http://purl.obolibrary.org/obo/GAZ_00056597 -->

    <owl:NamedIndividual rdf:about="http://purl.obolibrary.org/obo/GAZ_00056597">
        <obo:RO_0001025 rdf:resource="http://purl.obolibrary.org/obo/GAZ_00056596"/>
        <obo:IAO_0000115>A lava dome.</obo:IAO_0000115>
        <oboInOwl:hasOBONamespace>GAZ</oboInOwl:hasOBONamespace>
        <oboInOwl:id>GAZ:00056597</oboInOwl:id>
        <rdfs:label>Volcan Nuevo</rdfs:label>
    </owl:NamedIndividual>
    


    <!-- http://purl.obolibrary.org/obo/GAZ_00056598 -->

    <owl:NamedIndividual rdf:about="http://purl.obolibrary.org/obo/GAZ_00056598">
        <obo:RO_0001025 rdf:resource="http://purl.obolibrary.org/obo/GAZ_00056596"/>
        <obo:IAO_0000115>A stratovolcano.</obo:IAO_0000115>
        <oboInOwl:hasOBONamespace>GAZ</oboInOwl:hasOBONamespace>
        <oboInOwl:id>GAZ:00056598</oboInOwl:id>
        <rdfs:label>Volcan Viejo</rdfs:label>
    </owl:NamedIndividual>
    


    <!-- http://purl.obolibrary.org/obo/GAZ_00056599 -->

    <owl:NamedIndividual rdf:about="http://purl.obolibrary.org/obo/GAZ_00056599">
        <obo:RO_0001025 rdf:resource="http://purl.obolibrary.org/obo/GAZ_00056596"/>
        <obo:IAO_0000115>A stratovolcano.</obo:IAO_0000115>
        <oboInOwl:hasOBONamespace>GAZ</oboInOwl:hasOBONamespace>
        <oboInOwl:id>GAZ:00056599</oboInOwl:id>
        <rdfs:label>Volcan Nevado</rdfs:label>
    </owl:NamedIndividual>
    


    <!-- http://purl.obolibrary.org/obo/GAZ_00056601 -->

    <owl:NamedIndividual rdf:about="http://purl.obolibrary.org/obo/GAZ_00056601">
        <obo:RO_0001025 rdf:resource="http://purl.obolibrary.org/obo/GAZ_00136454"/>
        <obo:IAO_0000115>A Pleistocene to Holocene volcanic field located N of the Straits of Magellan, about 150 km NW of Punta Arenas. The 3000 km2 Pleistocene-to-Holocene Palei-Aike volcanic field straddles the Chile-Argentina border north of the Straits of Magellan, about 150 km NE of the town of Punta Arenas. The southernmost of the Patagonian basaltic plateau lavas, Palei-Aike contains lake-filled maars and basaltic scoria and spatter cones with associated fresh-looking lava flows. The distribution of maars and cones indicates that eruptions occurred along regional fissures oriented E-W and NW-SE. The earliest eruptions produced maars and associated lava flows that are now exposed only in river valleys. A second stage formed now-eroded spatter cones and soil-covered lava flows. The youngest cones and lava flows are found in the SE part of the volcanic field. The most recent volcanic event produced scoria and spatter cones and fresh lava flows not covered by soil.</obo:IAO_0000115>
        <oboInOwl:hasOBONamespace>GAZ</oboInOwl:hasOBONamespace>
        <oboInOwl:id>GAZ:00056601</oboInOwl:id>
        <rdfs:label>Pali-Aike Volcanic Field</rdfs:label>
    </owl:NamedIndividual>
    


    <!-- http://purl.obolibrary.org/obo/GAZ_00056602 -->

    <owl:NamedIndividual rdf:about="http://purl.obolibrary.org/obo/GAZ_00056602">
        <obo:RO_0001025 rdf:resource="http://purl.obolibrary.org/obo/GAZ_00136453"/>
        <obo:IAO_0000115>A Chilean stratovolcano located in the O&apos;Higgins Region, west of Caldera del Atuel. It is a small, 4850 m high volcano that is somewhat dissected by glaciers. A NE-flank cone, Andres, is postglacial in age and has produced andesitic lava flows. Palomo lies west of the massive Caldera del Atuel and was constructed within double calderas 3 and 5 km in diameter. The largely ice-covered Palomo has erupted basaltic-andesite to dacitic lava flows; a double crater indicates migration of activity to the NE. The youthful morphology of Palomo suggests a very recent, perhaps prehispanic, age.</obo:IAO_0000115>
        <oboInOwl:hasOBONamespace>GAZ</oboInOwl:hasOBONamespace>
        <oboInOwl:id>GAZ:00056602</oboInOwl:id>
        <rdfs:label>Volcan Palomo</rdfs:label>
    </owl:NamedIndividual>
    


    <!-- http://purl.obolibrary.org/obo/GAZ_00056604 -->

    <owl:NamedIndividual rdf:about="http://purl.obolibrary.org/obo/GAZ_00056604">
        <obo:RO_0001025 rdf:resource="http://purl.obolibrary.org/obo/GAZ_00136449"/>
        <obo:IAO_0000115>A stratovolcano located in El Loa Province, Antofagasta Region, Chile, and near the border with Bolivia. The summit of 5946 m high Paniri contains three craters separated by about 4 km along a NW-SE trend. The age of this andesitic-to-dacitic volcano was considered to be Pleistocene-Holocene.</obo:IAO_0000115>
        <oboInOwl:hasOBONamespace>GAZ</oboInOwl:hasOBONamespace>
        <oboInOwl:id>GAZ:00056604</oboInOwl:id>
        <rdfs:label>Cerro Paniri</rdfs:label>
    </owl:NamedIndividual>
    


    <!-- http://purl.obolibrary.org/obo/GAZ_00056605 -->

    <owl:NamedIndividual rdf:about="http://purl.obolibrary.org/obo/GAZ_00056605">
        <obo:IAO_0000115>A mountain range in the Ancash Region of Peru. It is part of the larger Andes range.</obo:IAO_0000115>
        <oboInOwl:hasOBONamespace>GAZ</oboInOwl:hasOBONamespace>
        <oboInOwl:id>GAZ:00056605</oboInOwl:id>
        <rdfs:label>Cordillera Blanca</rdfs:label>
    </owl:NamedIndividual>
    


    <!-- http://purl.obolibrary.org/obo/GAZ_00056606 -->

    <owl:NamedIndividual rdf:about="http://purl.obolibrary.org/obo/GAZ_00056606">
        <obo:RO_0001025 rdf:resource="http://purl.obolibrary.org/obo/GAZ_00056262"/>
        <oboInOwl:hasOBONamespace>GAZ</oboInOwl:hasOBONamespace>
        <oboInOwl:id>GAZ:00056606</oboInOwl:id>
        <rdfs:label>Cordillera Occidental of Peru</rdfs:label>
    </owl:NamedIndividual>
    


    <!-- http://purl.obolibrary.org/obo/GAZ_00056607 -->

    <owl:NamedIndividual rdf:about="http://purl.obolibrary.org/obo/GAZ_00056607">
        <obo:RO_0001025 rdf:resource="http://purl.obolibrary.org/obo/GAZ_00056261"/>
        <obo:IAO_0000115>A mountain range that is part of the Cordillera Oriental, one of three mountain ranges in the Andes Mountains of west central Peru. It extends over an area about 180 km long and 25-40 km wide, stretching in a NNW-SSE direction parallel to the Pacific coast, its ridge circa 60 km from the coastline. It is part of the Andean Sierra which inland borders on the Costa, the narrow strip of coastal deserts along the South American coast. In the north and east the cordillera is bordered by Rio Santa which crosses the coastal ridge at 8deg45minS and runs parallel to the Cordillera Negra for almost all its length. In the south the cordillera is bordered by Rio Pativilca at 10deg30minS. In the cordillera&apos;s central part near Huaraz, Rio Casma breaks through the cordillera&apos;s ridge. Rio Santa separates Cordillera Negra from Cordillera Blanca, a snow-covered range rising up to 6,768 m in the east. Cordillera Negra for most of the year has no snow although it rises to 5,000 m in its highest parts. Cordillera Negra intercepts the warmth from the coast, causing the line of perpetual snow sinking as low as 5,100 m in the Cordillera Blanca.</obo:IAO_0000115>
        <oboInOwl:hasOBONamespace>GAZ</oboInOwl:hasOBONamespace>
        <oboInOwl:id>GAZ:00056607</oboInOwl:id>
        <rdfs:label>Cordillera Negra</rdfs:label>
    </owl:NamedIndividual>
    


    <!-- http://purl.obolibrary.org/obo/GAZ_00056608 -->

    <owl:NamedIndividual rdf:about="http://purl.obolibrary.org/obo/GAZ_00056608">
        <obo:RO_0001025 rdf:resource="http://purl.obolibrary.org/obo/GAZ_00002931"/>
        <obo:IAO_0000115>A series of mountain ranges, or massif, in northwestern Venezuela. The Cordillera de Merida is a northeastern extension of the Andes Mountains. The ranges run southwest-northeast between the Venezuelan-Colombian border and the Venezuelan coastal range. The Tachira depression separates the Cordillera de Merida from the Cordillera Oriental, which forms the Colombia-Venezuela border. The ranges runs from southwest to northeast and parts lie within each of the following states: Tachira, Merida, Barinas, Trujillo, Portuguesa and Lara. The southeastern slopes are drained by tributaries of the Orinoco River, while the streams that drain the northwestern slopes empty into Lake Maracaibo. At the northeast tip of the massif lies the town of Barquisimeto and the headwaters of the River Cojedes. In the centre of the massif is the city of Merida. Two ranges of peaks lie on either side of the city, the Sierra de la Culata to the north and Sierra Nevada de Merida to the south. Pico Bolivar, at 4,981 m elevation, is the highest peak in Venezuela.</obo:IAO_0000115>
        <oboInOwl:hasOBONamespace>GAZ</oboInOwl:hasOBONamespace>
        <oboInOwl:id>GAZ:00056608</oboInOwl:id>
        <rdfs:label>Cordillera de Merida</rdfs:label>
    </owl:NamedIndividual>
    


    <!-- http://purl.obolibrary.org/obo/GAZ_00056668 -->

    <owl:NamedIndividual rdf:about="http://purl.obolibrary.org/obo/GAZ_00056668">
        <obo:RO_0001025 rdf:resource="http://purl.obolibrary.org/obo/GAZ_00136453"/>
        <obo:IAO_0000115>An elongated complex volcano along the Chile-Argentina border with several overlapping calderas. Activity began in the Pleistocene with construction of the basaltic-andesite to dacitic Volcan Azufre, followed by formation of basaltic and basaltic-andesite Volcan Planchon, 6 km to the north. About 11,500 years ago, much of Azufre and part of Planchon collapsed, forming the massive Rio Teno debris avalanche, which traveled 95 km to reach Chile&apos;s Central Valley. Subsequently, Volcan Planchon II was formed. The youngest volcano, andesitic and basaltic-andesite Volcan Peteroa, consists of scattered vents between Azufre and Planchan. Peteroa has been active into historical time and contains a small steaming crater lake.</obo:IAO_0000115>
        <oboInOwl:hasOBONamespace>GAZ</oboInOwl:hasOBONamespace>
        <oboInOwl:id>GAZ:00056668</oboInOwl:id>
        <rdfs:label>Planchon-Peteroa Volcano</rdfs:label>
    </owl:NamedIndividual>
    


    <!-- http://purl.obolibrary.org/obo/GAZ_00056672 -->

    <owl:NamedIndividual rdf:about="http://purl.obolibrary.org/obo/GAZ_00056672">
        <obo:RO_0001025 rdf:resource="http://purl.obolibrary.org/obo/GAZ_00136449"/>
        <obo:IAO_0000115>A stratovolcano located in the Antofagasta Region of Chile, immediately northeast of Cerro Pajonales and about 15 km west of the border with Argentina.</obo:IAO_0000115>
        <oboInOwl:hasOBONamespace>GAZ</oboInOwl:hasOBONamespace>
        <oboInOwl:id>GAZ:00056672</oboInOwl:id>
        <rdfs:label>Cerros Pular</rdfs:label>
    </owl:NamedIndividual>
    


    <!-- http://purl.obolibrary.org/obo/GAZ_00056673 -->

    <owl:NamedIndividual rdf:about="http://purl.obolibrary.org/obo/GAZ_00056673">
        <obo:RO_0001025 rdf:resource="http://purl.obolibrary.org/obo/GAZ_00056541"/>
        <obo:RO_0001025 rdf:resource="http://purl.obolibrary.org/obo/GAZ_00136449"/>
        <obo:IAO_0000115>A stratovolcano in northwestern Argentina, just east of the Chilean border.</obo:IAO_0000115>
        <oboInOwl:hasOBONamespace>GAZ</oboInOwl:hasOBONamespace>
        <oboInOwl:id>GAZ:00056673</oboInOwl:id>
        <rdfs:label>Volcan Aracar</rdfs:label>
    </owl:NamedIndividual>
    


    <!-- http://purl.obolibrary.org/obo/GAZ_00056685 -->

    <owl:NamedIndividual rdf:about="http://purl.obolibrary.org/obo/GAZ_00056685">
        <obo:RO_0001025 rdf:resource="http://purl.obolibrary.org/obo/GAZ_00136449"/>
        <obo:IAO_0000115>A stratovolcano on the border between Bolivia and Chile. It lies immediately north of Sairecabur complex and south of Tocorpuri. Intense fumarolic activity occurs at its summit. It is part of a large, roughly N-S-trending volcanic complex that covers an area of 600 sq km. Vigorous fumarolic activity is visible at the 5890 m high summit of Putana volcano from long distances. The main edifice, which formed primarily by lava effusion, consists of accumulated postglacial dacitic lava domes and flows mantling an older pre-Holocene volcano. The youngest basaltic andesite lava flows are viscous and rarely extend more than 3 km.</obo:IAO_0000115>
        <oboInOwl:hasOBONamespace>GAZ</oboInOwl:hasOBONamespace>
        <oboInOwl:id>GAZ:00056685</oboInOwl:id>
        <rdfs:label>Volcan Putana</rdfs:label>
    </owl:NamedIndividual>
    


    <!-- http://purl.obolibrary.org/obo/GAZ_00056686 -->

    <owl:NamedIndividual rdf:about="http://purl.obolibrary.org/obo/GAZ_00056686">
        <obo:RO_0001025 rdf:resource="http://purl.obolibrary.org/obo/GAZ_00136453"/>
        <obo:IAO_0000115>A chain of dominantly basaltic cinder cones erupted along two NE-SW-trending fissures at the head of Puyuhuapi fjord comprise the Volcanes de Puyuhuapi. The larger group of four cones lies on the western side of Puyuhuapi fjord and fed lava flows that traveled SE to the sea. The second lineament formed a chain of four smaller cones between the head of the fjord and Lake Risopatron to the north. The two fractures are related to the regional Liquine-Ofqui fault zone. The Puyuhuapi cinder cones are extremely well preserved, suggesting a very young age. A portion of the Puyuhuapi Volcanic Group form part of the Queulat National Park, specifically the area south of the Lake Risopatron.</obo:IAO_0000115>
        <oboInOwl:hasOBONamespace>GAZ</oboInOwl:hasOBONamespace>
        <oboInOwl:id>GAZ:00056686</oboInOwl:id>
        <rdfs:label>Volcanes de Puyuhuapi</rdfs:label>
    </owl:NamedIndividual>
    


    <!-- http://purl.obolibrary.org/obo/GAZ_00056687 -->

    <owl:NamedIndividual rdf:about="http://purl.obolibrary.org/obo/GAZ_00056687">
        <obo:RO_0001025 rdf:resource="http://purl.obolibrary.org/obo/GAZ_00136453"/>
        <obo:IAO_0000115>A stratovolcanoi located along the Chile-Argentina border at the southern end of a volcano group that includes the Pleistocene volcanoes of Marmolejo and Espiritu Santo. The glaciated 6109 m high Marmolejo stratovolcano is truncated by a 4 km wide caldera, breached to the NW, that has been the source of a massive debris avalanche. San Jose is a 5856 m high stratovolcano of Pleistocene-Holocene age with a broad 2 km x 0.5 km summit region containing overlapping and nested craters, pyroclastic cones, and blocky lava flows. Volcan la Engorda and Volcan Plantat, located SW of Marmolejo and NW of San Jose, have also been active during the Holocene. An 8 km-long lava flow traveled to the SW from the 1 km wide summit crater of Espiritu Santo volcano, which overlaps the southern slope of Marmolejo. Mild phreatomagmatic eruptions were recorded from San Jose in the 19th and 20th centuries.</obo:IAO_0000115>
        <oboInOwl:hasOBONamespace>GAZ</oboInOwl:hasOBONamespace>
        <oboInOwl:id>GAZ:00056687</oboInOwl:id>
        <rdfs:label>Volcan San Jose</rdfs:label>
    </owl:NamedIndividual>
    


    <!-- http://purl.obolibrary.org/obo/GAZ_00056688 -->

    <owl:NamedIndividual rdf:about="http://purl.obolibrary.org/obo/GAZ_00056688">
        <obo:RO_0001025 rdf:resource="http://purl.obolibrary.org/obo/GAZ_00136449"/>
        <obo:IAO_0000115>A stratovolcano located on the edge of the Atacama Desert, in Chile. San Pablo volcano is its neighbor to the east. The youngest cone of San Pedro was constructed within a large horseshoe-shaped escarpment left by the collapse of an older edifice, which produced a large debris avalanche to the west, perhaps accompanied by a major pumice eruption. Thick dacitic lava flows with steep-sided fronts mantle the upper portion of the younger cone.</obo:IAO_0000115>
        <oboInOwl:hasOBONamespace>GAZ</oboInOwl:hasOBONamespace>
        <oboInOwl:id>GAZ:00056688</oboInOwl:id>
        <rdfs:label>Volcan San Pedro</rdfs:label>
    </owl:NamedIndividual>
    


    <!-- http://purl.obolibrary.org/obo/GAZ_00056689 -->

    <owl:NamedIndividual rdf:about="http://purl.obolibrary.org/obo/GAZ_00056689">
        <rdf:type rdf:resource="http://purl.obolibrary.org/obo/ENVO_00000354"/>
        <obo:RO_0001025 rdf:resource="http://purl.obolibrary.org/obo/GAZ_00136449"/>
        <obo:IAO_0000115>A volcanic complex which lies in both Chile and Argentina. Some of the complex is of Holocene age, but there is also Pleistocene volcanism evident.</obo:IAO_0000115>
        <oboInOwl:hasOBONamespace>GAZ</oboInOwl:hasOBONamespace>
        <oboInOwl:id>GAZ:00056689</oboInOwl:id>
        <rdfs:label>Sierra Nevada de Lagunas Bravas Volcanic Complex</rdfs:label>
    </owl:NamedIndividual>
    


    <!-- http://purl.obolibrary.org/obo/GAZ_00056690 -->

    <owl:NamedIndividual rdf:about="http://purl.obolibrary.org/obo/GAZ_00056690">
        <obo:RO_0001025 rdf:resource="http://purl.obolibrary.org/obo/GAZ_00136449"/>
        <obo:IAO_0000115>A stratovolcano at the border of Argentina and Chile. The western rim of the volcano borders the Monturaqui Basin. It is a massive, 6051 m high dacitic stratovolcano that lies immediately north of the only railway line between the two countries. Socompa is the youngest and southernmost of a 6000 m high NE-SW-trending chain of volcanoes including Pular and Pajonales. In contrast to the latter two volcanoes, no glacial moraines have been observed on the youthful and relatively uneroded Socompa volcano. Collapse of the NW portion of Socompa volcano about 7200 years ago, during an eruption similar to that at Mount St. Helens in 1980, produced a 600 km2 debris-avalanche deposit that extends about 40 km from the summit and is one of the world&apos;s largest and best exposed. Post-collapse eruptions have constructed dacitic lava domes that have filled much of the head of the collapse scarp. No historical eruptions are known from Socompa.</obo:IAO_0000115>
        <oboInOwl:hasOBONamespace>GAZ</oboInOwl:hasOBONamespace>
        <oboInOwl:id>GAZ:00056690</oboInOwl:id>
        <rdfs:label>Volcan Socompa</rdfs:label>
    </owl:NamedIndividual>
    


    <!-- http://purl.obolibrary.org/obo/GAZ_00056693 -->

    <owl:NamedIndividual rdf:about="http://purl.obolibrary.org/obo/GAZ_00056693">
        <obo:RO_0001025 rdf:resource="http://purl.obolibrary.org/obo/GAZ_00136449"/>
        <obo:IAO_0000115>A large stratovolcano on the border between Argentina and Chile, west of Ojos del Salado. It consists of nine eruptive centers and is covered in light-colored rhyodacite pyroclastic flow deposits.</obo:IAO_0000115>
        <oboInOwl:hasOBONamespace>GAZ</oboInOwl:hasOBONamespace>
        <oboInOwl:id>GAZ:00056693</oboInOwl:id>
        <rdfs:label>Cerro Solo</rdfs:label>
    </owl:NamedIndividual>
    


    <!-- http://purl.obolibrary.org/obo/GAZ_00056694 -->

    <owl:NamedIndividual rdf:about="http://purl.obolibrary.org/obo/GAZ_00056694">
        <obo:IAO_0000115>A national park located in Chile&apos;s far north, in the Andean range. It encompasses an area of 1,379 km2 of altiplano and mountains, the latter consisting mainly of enormous volcanoes. Las Vicunas National Reserve is its neighbour to the south. Both protected areas, along with Salar de Surire Natural Monument, form Lauca Biosphere Reserve. The park borders Sajama National Park in Bolivia.</obo:IAO_0000115>
        <oboInOwl:hasOBONamespace>GAZ</oboInOwl:hasOBONamespace>
        <oboInOwl:id>GAZ:00056694</oboInOwl:id>
        <rdfs:label>Parque Nacional Lauca</rdfs:label>
    </owl:NamedIndividual>
    


    <!-- http://purl.obolibrary.org/obo/GAZ_00056695 -->

    <owl:NamedIndividual rdf:about="http://purl.obolibrary.org/obo/GAZ_00056695">
        <obo:RO_0001025 rdf:resource="http://purl.obolibrary.org/obo/GAZ_00056694"/>
        <obo:IAO_0000115>A brackish lake located in the Andean altiplano of the Parinacota Province, Arica-Parinacota Region, Chile. It lies 4 km northwest of Chungara Lake, which is one of the highest lakes in the world and is surrounded by several volcanoes, such as the group formed by the Nevados de Payachata (Parinacota and Pomerape), the Nevado Sajama and the Guallatiri. Laguna de Cotacotani is separated from the lake Chungara by a strip of volcanic rock and receives groundwater inflow from that lake, however its major sources are Benedicto Morales River and El Encuentro Creek. It empties through Lauca River into Coipasa Lake, in Bolivia.</obo:IAO_0000115>
        <oboInOwl:hasOBONamespace>GAZ</oboInOwl:hasOBONamespace>
        <oboInOwl:id>GAZ:00056695</oboInOwl:id>
        <rdfs:label>Laguna de Cotacotani</rdfs:label>
    </owl:NamedIndividual>
    


    <!-- http://purl.obolibrary.org/obo/GAZ_00056696 -->

    <owl:NamedIndividual rdf:about="http://purl.obolibrary.org/obo/GAZ_00056696">
        <obo:IAO_0000115>A nature reserve located in the Parinacota Province, Arica and Parinacota Region, Chile. The reserve lies immediately south of Lauca National Park and in its southern portion is contiguous to Salar de Surire Natural Monument, all of which form Lauca Biosphere Reserve.</obo:IAO_0000115>
        <oboInOwl:hasOBONamespace>GAZ</oboInOwl:hasOBONamespace>
        <oboInOwl:id>GAZ:00056696</oboInOwl:id>
        <rdfs:label>Reserva Nacional Las Vicunas</rdfs:label>
    </owl:NamedIndividual>
    


    <!-- http://purl.obolibrary.org/obo/GAZ_00056697 -->

    <owl:NamedIndividual rdf:about="http://purl.obolibrary.org/obo/GAZ_00056697">
        <obo:IAO_0000115>A protected place located in the Andes, in the Arica and Parinacota Region. It consists mainly of a salt flat and a number of small saline lakes. A World Biosphere Reserve.</obo:IAO_0000115>
        <oboInOwl:hasOBONamespace>GAZ</oboInOwl:hasOBONamespace>
        <oboInOwl:id>GAZ:00056697</oboInOwl:id>
        <rdfs:label>Monumento Natural Salar de Surire</rdfs:label>
    </owl:NamedIndividual>
    


    <!-- http://purl.obolibrary.org/obo/GAZ_00056698 -->

    <owl:NamedIndividual rdf:about="http://purl.obolibrary.org/obo/GAZ_00056698">
        <obo:RO_0001025 rdf:resource="http://purl.obolibrary.org/obo/GAZ_00056694"/>
        <obo:RO_0001025 rdf:resource="http://purl.obolibrary.org/obo/GAZ_00056697"/>
        <obo:IAO_0000115>A saline lake. A Ramsar Site.</obo:IAO_0000115>
        <oboInOwl:hasOBONamespace>GAZ</oboInOwl:hasOBONamespace>
        <oboInOwl:id>GAZ:00056698</oboInOwl:id>
        <rdfs:label>Salar de Surire</rdfs:label>
    </owl:NamedIndividual>
    


    <!-- http://purl.obolibrary.org/obo/GAZ_00056699 -->

    <owl:NamedIndividual rdf:about="http://purl.obolibrary.org/obo/GAZ_00056699">
        <rdf:type rdf:resource="http://purl.obolibrary.org/obo/ENVO_00000354"/>
        <obo:RO_0001025 rdf:resource="http://purl.obolibrary.org/obo/GAZ_00056694"/>
        <obo:RO_0001025 rdf:resource="http://purl.obolibrary.org/obo/GAZ_00136449"/>
        <obo:IAO_0000115>A volcanic complex, lying west of the main Andean chain, rises NE of the small town of Putre in northern Chile. The elongated volcanic massif, known locally as Nevados de Putre, consists of an initial andesitic stratovolcano and a long-term dacitic lava-dome complex. Taapaca overlies Pleistocene ignimbrite deposits and trends roughly E-W, with activity in general migrating to the SW during four principal periods of activity dating back at least 1.5 million years. At least three major edifice collapse events have produced debris-avalanche deposits, the youngest of which underlies Putre, the principal settlement of the northern Chilean Altiplano. Recent geological studies have shown that explosive activity at Taapaca with dome growth and associated block-and-ash flows and lahars has continued into the late Holocene. The youngest volcanic stage beginning about 9000 years ago produced the 5860 m high summit lava dome of the Putre Unit at the eastern and southern ends of the complex. The latest documented activity produced an ash layer dated at about 2000 years ago.</obo:IAO_0000115>
        <oboInOwl:hasOBONamespace>GAZ</oboInOwl:hasOBONamespace>
        <oboInOwl:id>GAZ:00056699</oboInOwl:id>
        <rdfs:label>Nevados de Putre Volcanic Complex</rdfs:label>
    </owl:NamedIndividual>
    


    <!-- http://purl.obolibrary.org/obo/GAZ_00056700 -->

    <owl:NamedIndividual rdf:about="http://purl.obolibrary.org/obo/GAZ_00056700">
        <obo:RO_0001025 rdf:resource="http://purl.obolibrary.org/obo/GAZ_00136449"/>
        <obo:IAO_0000115>A volcano located in Arica y Parinacota Region of Chile. A stratovolcano that overlies a flat-lying platform of ignimbrites at about 4200 m elevation forming the Arica Altiplano. The roughly conical volcano is covered by glaciers down to about 5500 m elevation, and an explosion crater lies on the NW side 300 m below the summit. Solfataric and fumarolic activity has been reported on the east side of the andesitic volcano.</obo:IAO_0000115>
        <oboInOwl:hasOBONamespace>GAZ</oboInOwl:hasOBONamespace>
        <oboInOwl:id>GAZ:00056700</oboInOwl:id>
        <rdfs:label>Volcan Tacora</rdfs:label>
    </owl:NamedIndividual>
    


    <!-- http://purl.obolibrary.org/obo/GAZ_00056701 -->

    <owl:NamedIndividual rdf:about="http://purl.obolibrary.org/obo/GAZ_00056701">
        <obo:RO_0001025 rdf:resource="http://purl.obolibrary.org/obo/GAZ_00136453"/>
        <obo:IAO_0000115>A stratovolcano located in the O&apos;Higgins Region of Chile. It is composed of at least seven Holocene scoria cones west of the Chile-Argentina border constructed along a NNE-SSW fissure over an eroded Pleistocene stratovolcano. The complex was constructed during three eruptive cycles dating back to the middle Pleistocene. The latest activity produced a series of youthful small stratovolcanoes and craters, of which the youngest appear to be Tinguiririca and Fray Carlos. Constant fumarolic activity occurs within and on the NW wall of the summit crater of Tinguiririca, and hot springs and fumaroles with sulfur deposits are found on the western flanks of the summit cones.</obo:IAO_0000115>
        <oboInOwl:hasOBONamespace>GAZ</oboInOwl:hasOBONamespace>
        <oboInOwl:id>GAZ:00056701</oboInOwl:id>
        <rdfs:label>Volcan Tinguiririca</rdfs:label>
    </owl:NamedIndividual>
    


    <!-- http://purl.obolibrary.org/obo/GAZ_00056702 -->

    <owl:NamedIndividual rdf:about="http://purl.obolibrary.org/obo/GAZ_00056702">
        <obo:RO_0001025 rdf:resource="http://purl.obolibrary.org/obo/GAZ_00136453"/>
        <obo:IAO_0000115>A massive stratovolcano dating to Pleistocene times. It lies on the border between Chile and the province of Mendoza, Argentina.</obo:IAO_0000115>
        <oboInOwl:hasOBONamespace>GAZ</oboInOwl:hasOBONamespace>
        <oboInOwl:id>GAZ:00056702</oboInOwl:id>
        <rdfs:label>Volcan Tupungato</rdfs:label>
    </owl:NamedIndividual>
    


    <!-- http://purl.obolibrary.org/obo/GAZ_00056703 -->

    <owl:NamedIndividual rdf:about="http://purl.obolibrary.org/obo/GAZ_00056703">
        <obo:RO_0001025 rdf:resource="http://purl.obolibrary.org/obo/GAZ_00136453"/>
        <obo:IAO_0000115>A stratovolcano located along the Chile-Argentina border about 90 km east of Santiago and immediately SW of the Pleistocene Tupungato volcano. Tupungatito consists of a group of 12 Holocene andesitic and basaltic andesite craters and a pyroclastic cone at the NW end of the 4 km wide, Pleistocene dacitic Nevado Sin Nombre caldera, which is filled by glaciers at its southern end and is breached to the NW. Lava flows from the northernmost vent have traveled down the NW flank breach. Tupungatito has produced frequent mild explosive eruptions during the 19th and 20th centuries.</obo:IAO_0000115>
        <oboInOwl:hasOBONamespace>GAZ</oboInOwl:hasOBONamespace>
        <oboInOwl:id>GAZ:00056703</oboInOwl:id>
        <rdfs:label>Volcan Tupungatito</rdfs:label>
    </owl:NamedIndividual>
    


    <!-- http://purl.obolibrary.org/obo/GAZ_00056704 -->

    <owl:NamedIndividual rdf:about="http://purl.obolibrary.org/obo/GAZ_00056704">
        <obo:RO_0001025 rdf:resource="http://purl.obolibrary.org/obo/GAZ_00136454"/>
        <obo:IAO_0000115>An eruptive center that is a subglacial dacitic volcano beneath the Patagonian Icecap west of the spectacular granitic spires of the Cerro Torre, Cerro Fitz Roy area. Only part of the older edifice rises above the surface of the icecap. Four large craters or calderas between 1.5 and 4 km in diameter are located along a N-S line. The 1988 eruption deposited ash and pumice on the Patagonian Icecap and produced a mudflow that reached Viedma Lake.</obo:IAO_0000115>
        <oboInOwl:hasOBONamespace>GAZ</oboInOwl:hasOBONamespace>
        <oboInOwl:id>GAZ:00056704</oboInOwl:id>
        <rdfs:label>Volcan Viedma</rdfs:label>
    </owl:NamedIndividual>
    


    <!-- http://purl.obolibrary.org/obo/GAZ_00056705 -->

    <owl:NamedIndividual rdf:about="http://purl.obolibrary.org/obo/GAZ_00056705">
        <obo:RO_0001025 rdf:resource="http://purl.obolibrary.org/obo/GAZ_00136449"/>
        <obo:IAO_0000115>A volcanic field in Argentina. The main type of volcanic edifice in the area are scoria cones. The field lies between the Salar de Antofalla volcanic field and the Cerro Galan caldera. The caldera lies west of Antofagasta de la Sierra and the other volcanic field to the east. The other prominent volcanic feature of the region, the peak Beltran, lies to the south-west of the field.</obo:IAO_0000115>
        <oboInOwl:hasOBONamespace>GAZ</oboInOwl:hasOBONamespace>
        <oboInOwl:id>GAZ:00056705</oboInOwl:id>
        <rdfs:label>Antofagasta de la Sierra Volcanic Field</rdfs:label>
    </owl:NamedIndividual>
    


    <!-- http://purl.obolibrary.org/obo/GAZ_00056706 -->

    <owl:NamedIndividual rdf:about="http://purl.obolibrary.org/obo/GAZ_00056706">
        <obo:RO_0001025 rdf:resource="http://purl.obolibrary.org/obo/GAZ_00056705"/>
        <obo:RO_0001025 rdf:resource="http://purl.obolibrary.org/obo/GAZ_00136449"/>
        <obo:IAO_0000115>A large and very remote stratovolcano in Catamarca Province in northwestern Argentina. It is located on the edge of the Puna de Atacama, a high desert plateau east of the Atacama Desert. It lies just west of the Salar de Antofalla, a large playa over 140 km in length.</obo:IAO_0000115>
        <oboInOwl:hasOBONamespace>GAZ</oboInOwl:hasOBONamespace>
        <oboInOwl:id>GAZ:00056706</oboInOwl:id>
        <rdfs:label>Volcan Antofalla</rdfs:label>
    </owl:NamedIndividual>
    


    <!-- http://purl.obolibrary.org/obo/GAZ_00056708 -->

    <owl:NamedIndividual rdf:about="http://purl.obolibrary.org/obo/GAZ_00056708">
        <obo:RO_0001025 rdf:resource="http://purl.obolibrary.org/obo/GAZ_00136453"/>
        <obo:IAO_0000115>A 30 x 45 km wide that lies just east of the Argentina-Chile border and 18 km SSW of the rim of Diamante caldera. The western rim of Caldera del Atuel in part follows the international border, and the headwaters of the Rio del Atuel drain to the SE through a wide breach in the caldera rim. The broad floor of the caldera is dotted with 15 dacitic lava domes and 25 basaltic-andesite to andesitic stratovolcanoes and cinder cones. A group of cones known as Las Lagrimas overlies the SW rim of the caldera, and Volcan Guanaqueros on the NE flank of the caldera is a group of young basaltic-to-andesitic cinder cones of possible historical age. The Volcan Overo complex in the NE part of the caldera and the Volcan Sosneado complex in the SE part of the caldera contain numerous very youthful basaltic-to-andesitic pyroclastic cones and lava flows. The Overo complex contains 20 centers, and lava flows of the Sosneado complex cover an area of 200 sq km.</obo:IAO_0000115>
        <oboInOwl:hasOBONamespace>GAZ</oboInOwl:hasOBONamespace>
        <oboInOwl:id>GAZ:00056708</oboInOwl:id>
        <rdfs:label>Caldera del Atuel</rdfs:label>
    </owl:NamedIndividual>
    


    <!-- http://purl.obolibrary.org/obo/GAZ_00056709 -->

    <owl:NamedIndividual rdf:about="http://purl.obolibrary.org/obo/GAZ_00056709">
        <obo:RO_0001025 rdf:resource="http://purl.obolibrary.org/obo/GAZ_00136449"/>
        <obo:IAO_0000115>A stratovolcano in Argentina. It lies within a 2.5 km wide caldera. The complex lies to the north of Falso Azufre volcano, which straddles the Chile/Argentina border. The summit of Cerro el Condor contains several ash cones and craters that have been the source of a number of pristine lava flows, one of which traveled 10 km to the west. Satellitic centers also abound; one on the east flank produced a fresh-looking lava flow that traveled 8 km to the east. The morphologically youthful lava flows and pristine summit crater imply a Holocene age (de Silva and Francis, 1991).</obo:IAO_0000115>
        <oboInOwl:hasOBONamespace>GAZ</oboInOwl:hasOBONamespace>
        <oboInOwl:id>GAZ:00056709</oboInOwl:id>
        <rdfs:label>Cerro El Condor</rdfs:label>
    </owl:NamedIndividual>
    


    <!-- http://purl.obolibrary.org/obo/GAZ_00056710 -->

    <owl:NamedIndividual rdf:about="http://purl.obolibrary.org/obo/GAZ_00056710">
        <obo:RO_0001025 rdf:resource="http://purl.obolibrary.org/obo/GAZ_00136449"/>
        <obo:IAO_0000115>A stratovolcano in northwestern Argentina about 120 km east of the main volcanic arc. Many youthful-looking flank lava flows were erupted from the well-preserved summit crater.</obo:IAO_0000115>
        <oboInOwl:hasOBONamespace>GAZ</oboInOwl:hasOBONamespace>
        <oboInOwl:id>GAZ:00056710</oboInOwl:id>
        <rdfs:label>Cerro Tuzgle</rdfs:label>
    </owl:NamedIndividual>
    


    <!-- http://purl.obolibrary.org/obo/GAZ_00056711 -->

    <owl:NamedIndividual rdf:about="http://purl.obolibrary.org/obo/GAZ_00056711">
        <obo:RO_0001025 rdf:resource="http://purl.obolibrary.org/obo/GAZ_00136453"/>
        <obo:IAO_0000115>A cinder cone in Argentina, located southeast of the massive stratovolcano of Tronador.</obo:IAO_0000115>
        <oboInOwl:hasOBONamespace>GAZ</oboInOwl:hasOBONamespace>
        <oboInOwl:id>GAZ:00056711</oboInOwl:id>
        <rdfs:label>Cerro Volcanico</rdfs:label>
    </owl:NamedIndividual>
    


    <!-- http://purl.obolibrary.org/obo/GAZ_00056712 -->

    <owl:NamedIndividual rdf:about="http://purl.obolibrary.org/obo/GAZ_00056712">
        <obo:RO_0001025 rdf:resource="http://purl.obolibrary.org/obo/GAZ_00136453"/>
        <obo:IAO_0000115>A small group of volcanoes north of the town of Buta Ranquil where the Rio Grande and Rio Barrancas join to form the Rio Colorado. Volcan Cochiquito is an alkaline basaltic stratovolcano of estimated Pleistocene-Holocene age north of the junction and has eight satellitic cones. Volcan Sillanegra is pyroclastic cone complex with two craters and basaltic aa lava flows located east of the Rio Grande. Its age was estimated to be Holocene (Gonzalez-Ferran, 1995). Volcan Ranquil del Sur is a small stratovolcano south of the Rio Barranca with an estimated Pleistocene-Holocene age that contains a 600-m-wide crater and produced andesitic pyroclastic material and lava flows.</obo:IAO_0000115>
        <oboInOwl:hasOBONamespace>GAZ</oboInOwl:hasOBONamespace>
        <oboInOwl:id>GAZ:00056712</oboInOwl:id>
        <rdfs:label>Cochiquito Volcanic Group</rdfs:label>
    </owl:NamedIndividual>
    


    <!-- http://purl.obolibrary.org/obo/GAZ_00056713 -->

    <owl:NamedIndividual rdf:about="http://purl.obolibrary.org/obo/GAZ_00056713">
        <obo:RO_0001025 rdf:resource="http://purl.obolibrary.org/obo/GAZ_00056712"/>
        <obo:IAO_0000115>A stratovolcano.</obo:IAO_0000115>
        <oboInOwl:hasOBONamespace>GAZ</oboInOwl:hasOBONamespace>
        <oboInOwl:id>GAZ:00056713</oboInOwl:id>
        <rdfs:label>Volcan Cochiquito</rdfs:label>
    </owl:NamedIndividual>
    


    <!-- http://purl.obolibrary.org/obo/GAZ_00056714 -->

    <owl:NamedIndividual rdf:about="http://purl.obolibrary.org/obo/GAZ_00056714">
        <obo:RO_0001025 rdf:resource="http://purl.obolibrary.org/obo/GAZ_00056712"/>
        <obo:IAO_0000115>A pyroclastic cone complex.</obo:IAO_0000115>
        <oboInOwl:hasOBONamespace>GAZ</oboInOwl:hasOBONamespace>
        <oboInOwl:id>GAZ:00056714</oboInOwl:id>
        <rdfs:label>Volcan Sillanegra</rdfs:label>
    </owl:NamedIndividual>
    


    <!-- http://purl.obolibrary.org/obo/GAZ_00056715 -->

    <owl:NamedIndividual rdf:about="http://purl.obolibrary.org/obo/GAZ_00056715">
        <obo:RO_0001025 rdf:resource="http://purl.obolibrary.org/obo/GAZ_00056712"/>
        <obo:IAO_0000115>A stratovolcano.</obo:IAO_0000115>
        <oboInOwl:hasOBONamespace>GAZ</oboInOwl:hasOBONamespace>
        <oboInOwl:id>GAZ:00056715</oboInOwl:id>
        <rdfs:label>Volcan Ranquil del Sur</rdfs:label>
    </owl:NamedIndividual>
    


    <!-- http://purl.obolibrary.org/obo/GAZ_00056716 -->

    <owl:NamedIndividual rdf:about="http://purl.obolibrary.org/obo/GAZ_00056716">
        <obo:RO_0001025 rdf:resource="http://purl.obolibrary.org/obo/GAZ_00136453"/>
        <obo:IAO_0000115>A stratovolcano located in the Argentine province of Neuquen. At least 14 dacitic lava domes and other eruptive centers were constructed within a broad 15 km wide caldera, and at least another 5 lie outside the caldera. The largest of the latter is Volcan Chanque-Mallin on the ESE flank. It is truncated by a 4 km wide caldera and contains a resurgent dome.</obo:IAO_0000115>
        <oboInOwl:hasOBONamespace>GAZ</oboInOwl:hasOBONamespace>
        <oboInOwl:id>GAZ:00056716</oboInOwl:id>
        <rdfs:label>Volcan Domuyo</rdfs:label>
    </owl:NamedIndividual>
    


    <!-- http://purl.obolibrary.org/obo/GAZ_00056717 -->

    <owl:NamedIndividual rdf:about="http://purl.obolibrary.org/obo/GAZ_00056717">
        <obo:RO_0001025 rdf:resource="http://purl.obolibrary.org/obo/GAZ_00136449"/>
        <obo:IAO_0000115>A caldera in Catamarca Province, Argentina.</obo:IAO_0000115>
        <oboInOwl:hasOBONamespace>GAZ</oboInOwl:hasOBONamespace>
        <oboInOwl:id>GAZ:00056717</oboInOwl:id>
        <rdfs:label>Galan Caldera</rdfs:label>
    </owl:NamedIndividual>
    


    <!-- http://purl.obolibrary.org/obo/GAZ_00056718 -->

    <owl:NamedIndividual rdf:about="http://purl.obolibrary.org/obo/GAZ_00056718">
        <obo:RO_0001025 rdf:resource="http://purl.obolibrary.org/obo/GAZ_00136453"/>
        <obo:IAO_0000115>A group of young basaltic stratovolcanoes in Argentina near the border with Chile, south of Lanin volcano. The Huanquihue volcano group consists of a NNE-SSW-trending chain of stratovolcanoes of Pleistocene age, some of which lie along the border. A Holocene compound cinder cone with three nested craters up to 400 m in diameter that occupied a valley NE of Cerro Huanquihue and a tuff cone constructed within glacial Lake Epulafquen lies at the northern end of the chain. Growth of this Holocene tuff cone, La Angostura (&quot;The Narrowing&quot;), created a peninsula that formed a narrow channel connecting Lake Epulafquen and Lake Huechulafquen. A very recent lava flow from the base of the Achin-Niellu cinder cone (also known as Cerro Escorial) traveled north into glacial Lago Epulafquen, forming a prominent lava delta. The Escorial lava flow is an extremely youthful flow that diverted local drainages and formed new lakes.</obo:IAO_0000115>
        <oboInOwl:hasOBONamespace>GAZ</oboInOwl:hasOBONamespace>
        <oboInOwl:id>GAZ:00056718</oboInOwl:id>
        <rdfs:label>Huanquihue Volcanic Group</rdfs:label>
    </owl:NamedIndividual>
    


    <!-- http://purl.obolibrary.org/obo/GAZ_00056721 -->

    <owl:NamedIndividual rdf:about="http://purl.obolibrary.org/obo/GAZ_00056721">
        <obo:RO_0001025 rdf:resource="http://purl.obolibrary.org/obo/GAZ_00136453"/>
        <obo:IAO_0000115>A massive hawaiian-style shield volcano in Argentina, located in the Reserva Provincial La Payunia of the Malargue Department, that lies 530 km from the oceanic trench. The elliptical alkaline caldera of Cerro Payun Matru is 8 x 10 km wide, and the high point of the massif is 3680 m high Cerro Payun stratovolcano, constructed over the SW flank of the shield. Post-caldera basaltic eruptions produced more than 300 eruptive centers, mostly along E-W-trending fissures that extend across the entire shield volcano. Fluid aa lava flows from a youthful concentration of vents on the west flank known as Los Volcanes traveled more than 10 km. Other vent clusters of the 5200 km2 Payun Matru volcanic field are found on the lower NE and southern flanks, and a lava flow from Volcan Santa Maria on the NW flank traveled 15 km to the NE. At least 30 trachyandesitic lava domes and basaltic lava flows were erupted contemporaneously with the basaltic fissure eruptions.</obo:IAO_0000115>
        <oboInOwl:hasOBONamespace>GAZ</oboInOwl:hasOBONamespace>
        <oboInOwl:id>GAZ:00056721</oboInOwl:id>
        <rdfs:label>Cerro Payun Matru</rdfs:label>
    </owl:NamedIndividual>
    


    <!-- http://purl.obolibrary.org/obo/GAZ_00056722 -->

    <owl:NamedIndividual rdf:about="http://purl.obolibrary.org/obo/GAZ_00056722">
        <obo:RO_0001025 rdf:resource="http://purl.obolibrary.org/obo/GAZ_00136449"/>
        <obo:IAO_0000115>A stratovolcano in Argentina. Cerro Peinado is one of the youngest volcanoes in the region. The upper part of the 5740 m high cone is blanketed by pyroclastic material. Two possible pyroclastic-flow lobes extend to the NW and north. Cerro Peinado contains an apron of pristine lava flows extending to 6 km. These were erupted from the main cone and from vents on the flank, including a prominent ESE-flank vent. Cerro Peinado is surrounded by small fields of cinder cones, maars, and pristine lava flows, located along N-S-trending faults, which are related to the Salar de Antofalla volcanic field.</obo:IAO_0000115>
        <oboInOwl:hasOBONamespace>GAZ</oboInOwl:hasOBONamespace>
        <oboInOwl:id>GAZ:00056722</oboInOwl:id>
        <rdfs:label>Cerro Peinado</rdfs:label>
    </owl:NamedIndividual>
    


    <!-- http://purl.obolibrary.org/obo/GAZ_00056725 -->

    <owl:NamedIndividual rdf:about="http://purl.obolibrary.org/obo/GAZ_00056725">
        <obo:RO_0001025 rdf:resource="http://purl.obolibrary.org/obo/GAZ_00136449"/>
        <obo:IAO_0000115>A caldera in Argentina, Catamarca Province. It is located 80 km SW of the much larger and better known Cerro Galan caldera. The Holocene Cerro Blanco del Robledo lava dome is located on the southern rim of the Robledo caldera (de Silva and Francis, 1991). Extensive rhyolitic pumice-fall deposits surround the dome. Well-preserved pyroclastic-flow deposits erupted prior to extrusion of Cerro Blanco are exposed on the floor of the caldera and on its NW flanks.</obo:IAO_0000115>
        <oboInOwl:hasOBONamespace>GAZ</oboInOwl:hasOBONamespace>
        <oboInOwl:id>GAZ:00056725</oboInOwl:id>
        <rdfs:label>Robledo Caldera</rdfs:label>
    </owl:NamedIndividual>
    


    <!-- http://purl.obolibrary.org/obo/GAZ_00056726 -->

    <owl:NamedIndividual rdf:about="http://purl.obolibrary.org/obo/GAZ_00056726">
        <obo:RO_0001025 rdf:resource="http://purl.obolibrary.org/obo/GAZ_00136449"/>
        <obo:IAO_0000115>A massive volcano complex in northwestern Argentina, located just southwest of Ojos del Salado. The 6660 m high summit of Cerro Tipas lies within Argentina, immediately south of the Chilean border. The Tipas volcanic complex of craters, cones, lava domes and lava flows covers an area of 25 sq km. It displays a youthful morphology, and its latest eruptions were considered by de Silva and Francis (1991) to be of Holocene age.</obo:IAO_0000115>
        <oboInOwl:hasOBONamespace>GAZ</oboInOwl:hasOBONamespace>
        <oboInOwl:id>GAZ:00056726</oboInOwl:id>
        <rdfs:label>Cerro Tipas</rdfs:label>
    </owl:NamedIndividual>
    


    <!-- http://purl.obolibrary.org/obo/GAZ_00056727 -->

    <owl:NamedIndividual rdf:about="http://purl.obolibrary.org/obo/GAZ_00056727">
        <obo:RO_0001025 rdf:resource="http://purl.obolibrary.org/obo/GAZ_00136453"/>
        <obo:IAO_0000115>A lava dome complex in Argentina NE of the Caldera del Agrio. This dacitic-andesitic lava-dome complex has two summit craters and a pyroclastic cone that fed andesitic lava flows that traveled to the east.</obo:IAO_0000115>
        <oboInOwl:hasOBONamespace>GAZ</oboInOwl:hasOBONamespace>
        <oboInOwl:id>GAZ:00056727</oboInOwl:id>
        <rdfs:label>Volcan Trocon</rdfs:label>
    </owl:NamedIndividual>
    


    <!-- http://purl.obolibrary.org/obo/GAZ_00056728 -->

    <owl:NamedIndividual rdf:about="http://purl.obolibrary.org/obo/GAZ_00056728">
        <obo:RO_0001025 rdf:resource="http://purl.obolibrary.org/obo/GAZ_00136453"/>
        <obo:IAO_0000115>A stratovolcano in western Argentina. It rises above the older caldera of the Volcan Negro del Tromen. The summit of Tromen is cut by two overlapping 3.5 km wide calderas. The Pleistocene Volcan Negro del Tromen, with a 5 km wide caldera, lies immediately north of Tromen, and lava flows from Tromen have partially overtopped the northern caldera rim. At the SSW end of this N-S-trending chain is Cerro Tilhue, of Pleistocene-Holocene age. Post-caldera vents at Tromen were constructed inside both calderas and on the flanks of the NE-most caldera. The youngest lava flows at Tromen originated from flanks vents and descended the north and NE sides of the andesitic-to-dacitic volcano. Holocene vents are also located in the Cerro Michico area on the lower NE flank.</obo:IAO_0000115>
        <oboInOwl:hasOBONamespace>GAZ</oboInOwl:hasOBONamespace>
        <oboInOwl:id>GAZ:00056728</oboInOwl:id>
        <rdfs:label>Volcan Tromen</rdfs:label>
    </owl:NamedIndividual>
    


    <!-- http://purl.obolibrary.org/obo/GAZ_00056729 -->

    <owl:NamedIndividual rdf:about="http://purl.obolibrary.org/obo/GAZ_00056729">
        <obo:RO_0001025 rdf:resource="http://purl.obolibrary.org/obo/GAZ_00008039"/>
        <obo:IAO_0000115>A delta, 200 km long that empties into the Gulf of Paria and the Atlantic Ocean, a very large delta (some 22.500 km2 and 370 km at its widest).</obo:IAO_0000115>
        <oboInOwl:hasOBONamespace>GAZ</oboInOwl:hasOBONamespace>
        <oboInOwl:id>GAZ:00056729</oboInOwl:id>
        <rdfs:label>Orinoco Delta</rdfs:label>
    </owl:NamedIndividual>
    


    <!-- http://purl.obolibrary.org/obo/GAZ_00056730 -->

    <owl:NamedIndividual rdf:about="http://purl.obolibrary.org/obo/GAZ_00056730">
        <obo:RO_0001025 rdf:resource="http://purl.obolibrary.org/obo/GAZ_00008039"/>
        <obo:IAO_0000115>A river, 959 km long with a well developed alluvial plain, flows in a Northeast direction, from Atures rapids down to Piacoa in front of Barrancas.</obo:IAO_0000115>
        <oboInOwl:hasOBONamespace>GAZ</oboInOwl:hasOBONamespace>
        <oboInOwl:id>GAZ:00056730</oboInOwl:id>
        <rdfs:label>Lower Orinoco</rdfs:label>
    </owl:NamedIndividual>
    


    <!-- http://purl.obolibrary.org/obo/GAZ_00056731 -->

    <owl:NamedIndividual rdf:about="http://purl.obolibrary.org/obo/GAZ_00056731">
        <obo:RO_0001025 rdf:resource="http://purl.obolibrary.org/obo/GAZ_00008039"/>
        <obo:IAO_0000115>A river, 242 km long, from its headwaters to the rapids Raudales de Guaharibos, flows through mountainous landscape in a northwesterly direction.</obo:IAO_0000115>
        <oboInOwl:hasOBONamespace>GAZ</oboInOwl:hasOBONamespace>
        <oboInOwl:id>GAZ:00056731</oboInOwl:id>
        <rdfs:label>Upper Orinoco</rdfs:label>
    </owl:NamedIndividual>
    


    <!-- http://purl.obolibrary.org/obo/GAZ_00056732 -->

    <owl:NamedIndividual rdf:about="http://purl.obolibrary.org/obo/GAZ_00056732">
        <obo:RO_0001025 rdf:resource="http://purl.obolibrary.org/obo/GAZ_00008039"/>
        <obo:IAO_0000115>A river, 750 km long, divided into two sectors, the first of which ca. 480 km long has a general westward direction down to the confluence with the Atabapo and Guaviare rivers at San Fernando de Atabapo; the second flows northward, for about 270 km, along the Venezuelan - Colombian border, flanked on both sides by the westernmost granitic upwellings of the Guiana Shield which impede the development of a flood plain, to the Atures rapids near the confluence with the Meta River at Puerto Carreno.</obo:IAO_0000115>
        <oboInOwl:hasOBONamespace>GAZ</oboInOwl:hasOBONamespace>
        <oboInOwl:id>GAZ:00056732</oboInOwl:id>
        <rdfs:label>Middle Orinoco</rdfs:label>
    </owl:NamedIndividual>
    


    <!-- http://purl.obolibrary.org/obo/GAZ_00056733 -->

    <owl:NamedIndividual rdf:about="http://purl.obolibrary.org/obo/GAZ_00056733">
        <rdf:type rdf:resource="http://purl.obolibrary.org/obo/ENVO_00000106"/>
        <obo:RO_0001025 rdf:resource="http://purl.obolibrary.org/obo/GAZ_00002931"/>
        <obo:IAO_0000115>A range of mountains in Venezuela, which run east to west along the country&apos;s northern coast. In the east they follow the border between the states of Vargas and Miranda. They then pass through the states of Aragua and Carabobo, and the eastern part of the State of Yaracuy, and they terminate south of the Yaracuy river in the northern part of the State of Cojedes.</obo:IAO_0000115>
        <oboInOwl:hasOBONamespace>GAZ</oboInOwl:hasOBONamespace>
        <oboInOwl:id>GAZ:00056733</oboInOwl:id>
        <rdfs:label>Cordillera de la Costa Central</rdfs:label>
    </owl:NamedIndividual>
    


    <!-- http://purl.obolibrary.org/obo/GAZ_00056736 -->

    <owl:NamedIndividual rdf:about="http://purl.obolibrary.org/obo/GAZ_00056736">
        <rdf:type rdf:resource="http://purl.obolibrary.org/obo/ENVO_00000104"/>
        <obo:RO_0001025 rdf:resource="http://purl.obolibrary.org/obo/GAZ_00002931"/>
        <obo:IAO_0000115>A basin in Western Venezuela. It is a prolific, oil-producing sedimentary basin. The basin is bounded on the north by the Oca Fault which separates it from the Caribbean Sea. The remaining sides of the basin are bounded by a branching in the northern Andes Mountains termed the Sierra de Perija (to the west) and the Merida Andes (to the south and east). The city of Maracaibo, Venezuela is located in the northern central part of the basin on the shore of Lake Maracaibo, which occupies the central part of basin.</obo:IAO_0000115>
        <oboInOwl:hasOBONamespace>GAZ</oboInOwl:hasOBONamespace>
        <oboInOwl:id>GAZ:00056736</oboInOwl:id>
        <rdfs:label>Maracaibo Basin</rdfs:label>
    </owl:NamedIndividual>
    


    <!-- http://purl.obolibrary.org/obo/GAZ_00056737 -->

    <owl:NamedIndividual rdf:about="http://purl.obolibrary.org/obo/GAZ_00056737">
        <obo:RO_0001025 rdf:resource="http://purl.obolibrary.org/obo/GAZ_00002931"/>
        <obo:RO_0001025 rdf:resource="http://purl.obolibrary.org/obo/GAZ_00056263"/>
        <obo:IAO_0000115>A mountain range, an extension of the eastern Andean branch (Cordillera Oriental), in northern South America, between Colombia and Venezuela, ending further north in the Guajira Desert, a total distance of about 310 km. It separates the Maracaibo Basin from the Cesar River valley.</obo:IAO_0000115>
        <oboInOwl:hasOBONamespace>GAZ</oboInOwl:hasOBONamespace>
        <oboInOwl:id>GAZ:00056737</oboInOwl:id>
        <rdfs:label>Serrania del Perija</rdfs:label>
    </owl:NamedIndividual>
    


    <!-- http://purl.obolibrary.org/obo/GAZ_00056738 -->

    <owl:NamedIndividual rdf:about="http://purl.obolibrary.org/obo/GAZ_00056738">
        <obo:RO_0001025 rdf:resource="http://purl.obolibrary.org/obo/GAZ_00136449"/>
        <obo:IAO_0000115>A geothermal field at Puchuldiza volcano, west of Salar Coipasa, is surrounded by Plio-Pleistocene volcanoes.</obo:IAO_0000115>
        <oboInOwl:hasOBONamespace>GAZ</oboInOwl:hasOBONamespace>
        <oboInOwl:id>GAZ:00056738</oboInOwl:id>
        <rdfs:label>Puchuldiza Geyser Field</rdfs:label>
    </owl:NamedIndividual>
    


    <!-- http://purl.obolibrary.org/obo/GAZ_00056762 -->

    <owl:NamedIndividual rdf:about="http://purl.obolibrary.org/obo/GAZ_00056762">
        <obo:RO_0001025 rdf:resource="http://purl.obolibrary.org/obo/GAZ_00056738"/>
        <obo:IAO_0000115>A stratovolcano.</obo:IAO_0000115>
        <oboInOwl:hasOBONamespace>GAZ</oboInOwl:hasOBONamespace>
        <oboInOwl:id>GAZ:00056762</oboInOwl:id>
        <rdfs:label>Cerro Guaillane</rdfs:label>
    </owl:NamedIndividual>
    


    <!-- http://purl.obolibrary.org/obo/GAZ_00056763 -->

    <owl:NamedIndividual rdf:about="http://purl.obolibrary.org/obo/GAZ_00056763">
        <obo:IAO_0000115>Two small youthful-looking maars are located in the Central Altiplano of Bolivia, north of Salar de Uyuni and east of Salar de Coipasa. Laguna Jayu Khota, initially considered to be a meteorite impact crater, was formed by basaltic-trachyandesite explosive volcanism. Nekhe Khota maar lies to the SW of Jayu Khota.</obo:IAO_0000115>
        <oboInOwl:hasOBONamespace>GAZ</oboInOwl:hasOBONamespace>
        <oboInOwl:id>GAZ:00056763</oboInOwl:id>
        <rdfs:label>Laguna Jayu Khota</rdfs:label>
    </owl:NamedIndividual>
    


    <!-- http://purl.obolibrary.org/obo/GAZ_00056764 -->

    <owl:NamedIndividual rdf:about="http://purl.obolibrary.org/obo/GAZ_00056764">
        <rdf:type rdf:resource="http://purl.obolibrary.org/obo/ENVO_00000354"/>
        <obo:RO_0001025 rdf:resource="http://purl.obolibrary.org/obo/GAZ_00136449"/>
        <obo:IAO_0000115>A volcanic complex, a 15 km-long E-W ridge forming the border between Chile and Bolivia. It is comprised of several stratovolcanoes with Holocene lava flows. Andesitic-dacitic lava flows extend as far as 5 km north from the active crater of Volcan Olca and to the north and west from vents farther to the west. Olca is flanked on the west by Cerro Michincha and on the east by Volcan Paruma, which is immediately west of the higher pre-Holocene Cerro Paruma volcano. Volcan Paruma has been the source of conspicuous fresh lava flows, one of which extends 7 km to the SE. Volcan Paruma has displayed persistent fumarolic activity in recent years. The only known historical activity from the Olca-Paruma complex was a flank eruption of unspecified character between 1865 and 1867.</obo:IAO_0000115>
        <oboInOwl:hasOBONamespace>GAZ</oboInOwl:hasOBONamespace>
        <oboInOwl:id>GAZ:00056764</oboInOwl:id>
        <rdfs:label>Olca-Paruma Volcanic Complex</rdfs:label>
    </owl:NamedIndividual>
    


    <!-- http://purl.obolibrary.org/obo/GAZ_00056765 -->

    <owl:NamedIndividual rdf:about="http://purl.obolibrary.org/obo/GAZ_00056765">
        <obo:RO_0001025 rdf:resource="http://purl.obolibrary.org/obo/GAZ_00056764"/>
        <obo:IAO_0000115>A stratovolcano.</obo:IAO_0000115>
        <oboInOwl:hasOBONamespace>GAZ</oboInOwl:hasOBONamespace>
        <oboInOwl:id>GAZ:00056765</oboInOwl:id>
        <rdfs:label>Volcan Paruma</rdfs:label>
    </owl:NamedIndividual>
    


    <!-- http://purl.obolibrary.org/obo/GAZ_00056766 -->

    <owl:NamedIndividual rdf:about="http://purl.obolibrary.org/obo/GAZ_00056766">
        <obo:RO_0001025 rdf:resource="http://purl.obolibrary.org/obo/GAZ_00056486"/>
        <obo:IAO_0000115>A dacitic lava-dome complex occupying the lower western flank of the Cerro del Azufre.</obo:IAO_0000115>
        <oboInOwl:hasOBONamespace>GAZ</oboInOwl:hasOBONamespace>
        <oboInOwl:id>GAZ:00056766</oboInOwl:id>
        <rdfs:label>Chanka Volcano</rdfs:label>
    </owl:NamedIndividual>
    


    <!-- http://purl.obolibrary.org/obo/GAZ_00056767 -->

    <owl:NamedIndividual rdf:about="http://purl.obolibrary.org/obo/GAZ_00056767">
        <obo:RO_0001025 rdf:resource="http://purl.obolibrary.org/obo/GAZ_00136449"/>
        <obo:IAO_0000115>An elongated fissure-controlled volcanic massif extending between the Pastos Grandes caldera and Laguna Colorada in Bolivia. More than 50 craters, small stratovolcanoes, and lava domes are located along four fissures covering an area of 230 sq km. Eight small andesitic-to-dacitic stratovolcanoes with craters between 0.2 and 1.5 km width are located along the southernmost fissure. A second fissure, oriented NW-SE and 10 km long, contains ten volcanic centers with craters with widths between 0.2 and 1.2 km. A third fissure, trending NE, produced 7 rhyodacitic lava domes. Activity has migrated to the north, with the youngest fissure, on the NW side of the complex, being of probable Holocene age (Gonzalez-Ferran, 1995). This NW-trending fissure, 7 km long, contains 27 small basaltic-andesite craters.</obo:IAO_0000115>
        <oboInOwl:hasOBONamespace>GAZ</oboInOwl:hasOBONamespace>
        <oboInOwl:id>GAZ:00056767</oboInOwl:id>
        <rdfs:label>Volcan de Jorcada</rdfs:label>
    </owl:NamedIndividual>
    


    <!-- http://purl.obolibrary.org/obo/GAZ_00056768 -->

    <owl:NamedIndividual rdf:about="http://purl.obolibrary.org/obo/GAZ_00056768">
        <rdf:type rdf:resource="http://purl.obolibrary.org/obo/ENVO_00000408"/>
        <obo:RO_0001025 rdf:resource="http://purl.obolibrary.org/obo/GAZ_00136449"/>
        <obo:IAO_0000115>A fissure vent whose laval effusions were considered to have occurred during the Holocene (Kussmaul et al., 1977). De Silva stated that volcanism in this area is pre-Holocene.</obo:IAO_0000115>
        <oboInOwl:hasOBONamespace>GAZ</oboInOwl:hasOBONamespace>
        <oboInOwl:id>GAZ:00056768</oboInOwl:id>
        <rdfs:label>Quetena Fissure Vent</rdfs:label>
    </owl:NamedIndividual>
    


    <!-- http://purl.obolibrary.org/obo/GAZ_00056769 -->

    <owl:NamedIndividual rdf:about="http://purl.obolibrary.org/obo/GAZ_00056769">
        <obo:RO_0001025 rdf:resource="http://purl.obolibrary.org/obo/GAZ_00136449"/>
        <obo:IAO_0000115>One of several stratovolcanoes located east of the vigorous Geisers del Tatio geothermal field. Lava flows at the base of the volcano are dacitic, while those at the upper part are andesitic-to-dacitic.</obo:IAO_0000115>
        <oboInOwl:hasOBONamespace>GAZ</oboInOwl:hasOBONamespace>
        <oboInOwl:id>GAZ:00056769</oboInOwl:id>
        <rdfs:label>El Volcan</rdfs:label>
    </owl:NamedIndividual>
    


    <!-- http://purl.obolibrary.org/obo/GAZ_00056770 -->

    <owl:NamedIndividual rdf:about="http://purl.obolibrary.org/obo/GAZ_00056770">
        <obo:RO_0001025 rdf:resource="http://purl.obolibrary.org/obo/GAZ_00136449"/>
        <obo:IAO_0000115>A group of N-S-trending rhyodacitic lava domes that straddles the Chile-Bolivia border. The 10 km-long chain is located immediately east of the Purico pyroclastic shield. There is some evidence for Holocene activity, and the youngest domes appear to be north of the summit crater of the dome complex (de Silva and Francis, 1991). A well-defined summit crater was the source of the largest lava flows, which traveled 3 km to the SW. There are no records of historical activity from Guayaques volcano.</obo:IAO_0000115>
        <oboInOwl:hasOBONamespace>GAZ</oboInOwl:hasOBONamespace>
        <oboInOwl:id>GAZ:00056770</oboInOwl:id>
        <rdfs:label>Cerros de Guayaques</rdfs:label>
    </owl:NamedIndividual>
    


    <!-- http://purl.obolibrary.org/obo/GAZ_00056771 -->

    <owl:NamedIndividual rdf:about="http://purl.obolibrary.org/obo/GAZ_00056771">
        <obo:RO_0001025 rdf:resource="http://purl.obolibrary.org/obo/GAZ_00136449"/>
        <obo:IAO_0000115>A 5631 m high andesitic-dacitic stratovolcano that was constructed on an uplifted block of welded ignimbrites. The most recent activity produced pristine silicic lava flows of probable Holocene age, the largest of which covers a 7 km2 area on the saddle between Colachi and the neighboring volcano of Acamarachi.</obo:IAO_0000115>
        <oboInOwl:hasOBONamespace>GAZ</oboInOwl:hasOBONamespace>
        <oboInOwl:id>GAZ:00056771</oboInOwl:id>
        <rdfs:label>Volcan Colachi</rdfs:label>
    </owl:NamedIndividual>
    


    <!-- http://purl.obolibrary.org/obo/GAZ_00056772 -->

    <owl:NamedIndividual rdf:about="http://purl.obolibrary.org/obo/GAZ_00056772">
        <obo:RO_0001025 rdf:resource="http://purl.obolibrary.org/obo/GAZ_00136449"/>
        <obo:IAO_0000115>A 5464 m high stratovolcano located west of Colachi volcano and is one of a cluster of young stratovolcanoes north and east of Lascar volcano.</obo:IAO_0000115>
        <oboInOwl:hasOBONamespace>GAZ</oboInOwl:hasOBONamespace>
        <oboInOwl:id>GAZ:00056772</oboInOwl:id>
        <rdfs:label>Volcan Laguna Verde</rdfs:label>
    </owl:NamedIndividual>
    


    <!-- http://purl.obolibrary.org/obo/GAZ_00056773 -->

    <owl:NamedIndividual rdf:about="http://purl.obolibrary.org/obo/GAZ_00056773">
        <obo:RO_0001025 rdf:resource="http://purl.obolibrary.org/obo/GAZ_00056559"/>
        <obo:IAO_0000115>A large basaltic-andesite to dacitic volcanic complex south of Laguna Miscanti. The 5910 m high summit of the volcano is cut by three overlapping, E-W-trending craters. Larger craters, partially filled by lava domes and flows, are located west and NE of the summit. A prominent lava flow extends NW-ward from the summit to the lower flanks, separating Laguna Miniques from Laguna Miscanti.</obo:IAO_0000115>
        <oboInOwl:hasOBONamespace>GAZ</oboInOwl:hasOBONamespace>
        <oboInOwl:id>GAZ:00056773</oboInOwl:id>
        <rdfs:label>Volcan Miniques</rdfs:label>
    </owl:NamedIndividual>
    


    <!-- http://purl.obolibrary.org/obo/GAZ_00056774 -->

    <owl:NamedIndividual rdf:about="http://purl.obolibrary.org/obo/GAZ_00056774">
        <obo:RO_0001025 rdf:resource="http://purl.obolibrary.org/obo/GAZ_00136449"/>
        <oboInOwl:hasOBONamespace>GAZ</oboInOwl:hasOBONamespace>
        <oboInOwl:id>GAZ:00056774</oboInOwl:id>
        <rdfs:label>Cordon de Tujle</rdfs:label>
    </owl:NamedIndividual>
    


    <!-- http://purl.obolibrary.org/obo/GAZ_00056775 -->

    <owl:NamedIndividual rdf:about="http://purl.obolibrary.org/obo/GAZ_00056775">
        <obo:RO_0001025 rdf:resource="http://purl.obolibrary.org/obo/GAZ_00056774"/>
        <obo:IAO_0000115>A Holocene maar with a 60-m-deep crater. The maar is located SE of the Salar de Atacama, north of Cerro Toloncha.</obo:IAO_0000115>
        <oboInOwl:hasOBONamespace>GAZ</oboInOwl:hasOBONamespace>
        <oboInOwl:id>GAZ:00056775</oboInOwl:id>
        <rdfs:label>Cerro Tujle</rdfs:label>
    </owl:NamedIndividual>
    


    <!-- http://purl.obolibrary.org/obo/GAZ_00056776 -->

    <owl:NamedIndividual rdf:about="http://purl.obolibrary.org/obo/GAZ_00056776">
        <obo:RO_0001025 rdf:resource="http://purl.obolibrary.org/obo/GAZ_00136449"/>
        <obo:IAO_0000115>Two small stratovolcanoes that lie about 3 km apart in the Callejon de Tilocalar area. The volcanoes overlie Pliocene ignimbrites and were considered to be of Pleistocene-Holocene age by Gonzalez-Ferran (1995). The larger volcano, Tilocalar Sur, lies about 3.5 km SW of the northern volcano, Tilocalar Norte. Four basaltic-andesite to andesitic lava flows originated from 3116 m high Tilocalar Sur, and an explosion crater lies a km to the south. The 3040 m high Tilocalar Norte lies near the eastern wall of the Callejon de Tilocalar and produced lava flows that traveled primarily to the north.</obo:IAO_0000115>
        <oboInOwl:hasOBONamespace>GAZ</oboInOwl:hasOBONamespace>
        <oboInOwl:id>GAZ:00056776</oboInOwl:id>
        <rdfs:label>Volcanes de Tilocalar</rdfs:label>
    </owl:NamedIndividual>
    


    <!-- http://purl.obolibrary.org/obo/GAZ_00056777 -->

    <owl:NamedIndividual rdf:about="http://purl.obolibrary.org/obo/GAZ_00056777">
        <obo:RO_0001025 rdf:resource="http://purl.obolibrary.org/obo/GAZ_00056776"/>
        <oboInOwl:hasOBONamespace>GAZ</oboInOwl:hasOBONamespace>
        <oboInOwl:id>GAZ:00056777</oboInOwl:id>
        <rdfs:label>Tilocalar Sud</rdfs:label>
    </owl:NamedIndividual>
    


    <!-- http://purl.obolibrary.org/obo/GAZ_00056778 -->

    <owl:NamedIndividual rdf:about="http://purl.obolibrary.org/obo/GAZ_00056778">
        <obo:RO_0001025 rdf:resource="http://purl.obolibrary.org/obo/GAZ_00056776"/>
        <oboInOwl:hasOBONamespace>GAZ</oboInOwl:hasOBONamespace>
        <oboInOwl:id>GAZ:00056778</oboInOwl:id>
        <rdfs:label>Tilocalar Norte</rdfs:label>
    </owl:NamedIndividual>
    


    <!-- http://purl.obolibrary.org/obo/GAZ_00056779 -->

    <owl:NamedIndividual rdf:about="http://purl.obolibrary.org/obo/GAZ_00056779">
        <obo:RO_0001025 rdf:resource="http://purl.obolibrary.org/obo/GAZ_00136449"/>
        <obo:IAO_0000115>A group of cinder cones and compound andesitic lava flows in what was interpreted to be a Holocene volcanic field west of the Cordon de Pular, however, did not consider El Negrillar to be of Holocene age. This volcanic field lies about 20 km north of Socompa volcano. The major Holocene debris avalanche from Socompa abuts the western margin of El Negrillar lava flows.</obo:IAO_0000115>
        <oboInOwl:hasOBONamespace>GAZ</oboInOwl:hasOBONamespace>
        <oboInOwl:id>GAZ:00056779</oboInOwl:id>
        <rdfs:label>El Negrillar Cinder Cones</rdfs:label>
    </owl:NamedIndividual>
    


    <!-- http://purl.obolibrary.org/obo/GAZ_00056780 -->

    <owl:NamedIndividual rdf:about="http://purl.obolibrary.org/obo/GAZ_00056780">
        <rdf:type rdf:resource="http://purl.obolibrary.org/obo/ENVO_00000398"/>
        <obo:RO_0001025 rdf:resource="http://purl.obolibrary.org/obo/GAZ_00136449"/>
        <obo:IAO_0000115>A cone and lava flow complex that covers a roughly 16 km area along the SW margin of the Atacama basin. This basaltic-andesite volcanic field, distinct from El Negrillar (north of Socompa), lies WSW of Socompa volcano between the Sierra San Juan and Sierra Almeida.</obo:IAO_0000115>
        <oboInOwl:hasOBONamespace>GAZ</oboInOwl:hasOBONamespace>
        <oboInOwl:id>GAZ:00056780</oboInOwl:id>
        <rdfs:label>La Negrillar</rdfs:label>
    </owl:NamedIndividual>
    


    <!-- http://purl.obolibrary.org/obo/GAZ_00056781 -->

    <owl:NamedIndividual rdf:about="http://purl.obolibrary.org/obo/GAZ_00056781">
        <obo:RO_0001025 rdf:resource="http://purl.obolibrary.org/obo/GAZ_00056510"/>
        <oboInOwl:hasOBONamespace>GAZ</oboInOwl:hasOBONamespace>
        <oboInOwl:id>GAZ:00056781</oboInOwl:id>
        <rdfs:label>Cerro Falso Azufre</rdfs:label>
    </owl:NamedIndividual>
    


    <!-- http://purl.obolibrary.org/obo/GAZ_00056782 -->

    <owl:NamedIndividual rdf:about="http://purl.obolibrary.org/obo/GAZ_00056782">
        <obo:RO_0001025 rdf:resource="http://purl.obolibrary.org/obo/GAZ_00056498"/>
        <obo:IAO_0000115>A cinder cone located 7 km north of Copiapo.</obo:IAO_0000115>
        <oboInOwl:hasOBONamespace>GAZ</oboInOwl:hasOBONamespace>
        <oboInOwl:id>GAZ:00056782</oboInOwl:id>
        <rdfs:label>Volcan San Roman</rdfs:label>
    </owl:NamedIndividual>
    


    <!-- http://purl.obolibrary.org/obo/GAZ_00057296 -->

    <owl:NamedIndividual rdf:about="http://purl.obolibrary.org/obo/GAZ_00057296">
        <rdf:type rdf:resource="http://purl.obolibrary.org/obo/ENVO_00000398"/>
        <obo:RO_0001025 rdf:resource="http://purl.obolibrary.org/obo/GAZ_00056555"/>
        <obo:IAO_0000115>A Pleistocene cone on the SW rim of Maipo Volcano.</obo:IAO_0000115>
        <oboInOwl:hasOBONamespace>GAZ</oboInOwl:hasOBONamespace>
        <oboInOwl:id>GAZ:00057296</oboInOwl:id>
        <rdfs:label>Volcan Don Casimiro</rdfs:label>
    </owl:NamedIndividual>
    


    <!-- http://purl.obolibrary.org/obo/GAZ_00057297 -->

    <owl:NamedIndividual rdf:about="http://purl.obolibrary.org/obo/GAZ_00057297">
        <rdf:type rdf:resource="http://purl.obolibrary.org/obo/ENVO_00000398"/>
        <obo:RO_0001025 rdf:resource="http://purl.obolibrary.org/obo/GAZ_00056555"/>
        <obo:IAO_0000115>A Pleistocene cone on the SW flank of Maipo Volcano.</obo:IAO_0000115>
        <oboInOwl:hasOBONamespace>GAZ</oboInOwl:hasOBONamespace>
        <oboInOwl:id>GAZ:00057297</oboInOwl:id>
        <rdfs:label>Cerro Listado</rdfs:label>
    </owl:NamedIndividual>
    


    <!-- http://purl.obolibrary.org/obo/GAZ_00057298 -->

    <owl:NamedIndividual rdf:about="http://purl.obolibrary.org/obo/GAZ_00057298">
        <obo:RO_0001025 rdf:resource="http://purl.obolibrary.org/obo/GAZ_00056708"/>
        <obo:IAO_0000115>Cinder cones that overlie the SW rim of Caldera del Atuel.</obo:IAO_0000115>
        <oboInOwl:hasOBONamespace>GAZ</oboInOwl:hasOBONamespace>
        <oboInOwl:id>GAZ:00057298</oboInOwl:id>
        <rdfs:label>Las Lagrimas</rdfs:label>
    </owl:NamedIndividual>
    


    <!-- http://purl.obolibrary.org/obo/GAZ_00057299 -->

    <owl:NamedIndividual rdf:about="http://purl.obolibrary.org/obo/GAZ_00057299">
        <obo:RO_0001025 rdf:resource="http://purl.obolibrary.org/obo/GAZ_00056708"/>
        <obo:IAO_0000115>A stratovolcano in the NE part of the Caldera del Atuel.</obo:IAO_0000115>
        <oboInOwl:hasOBONamespace>GAZ</oboInOwl:hasOBONamespace>
        <oboInOwl:id>GAZ:00057299</oboInOwl:id>
        <rdfs:label>Volcan Overo</rdfs:label>
    </owl:NamedIndividual>
    


    <!-- http://purl.obolibrary.org/obo/GAZ_00057300 -->

    <owl:NamedIndividual rdf:about="http://purl.obolibrary.org/obo/GAZ_00057300">
        <obo:RO_0001025 rdf:resource="http://purl.obolibrary.org/obo/GAZ_00056708"/>
        <obo:IAO_0000115>A cinder cone the NE flank of the Caldera del Atuel.</obo:IAO_0000115>
        <oboInOwl:hasOBONamespace>GAZ</oboInOwl:hasOBONamespace>
        <oboInOwl:id>GAZ:00057300</oboInOwl:id>
        <rdfs:label>Volcan Guanaqueros</rdfs:label>
    </owl:NamedIndividual>
    


    <!-- http://purl.obolibrary.org/obo/GAZ_00057301 -->

    <owl:NamedIndividual rdf:about="http://purl.obolibrary.org/obo/GAZ_00057301">
        <obo:RO_0001025 rdf:resource="http://purl.obolibrary.org/obo/GAZ_00056708"/>
        <obo:IAO_0000115>A stratovolcano in the SE part of the Caldera del Atuel.</obo:IAO_0000115>
        <oboInOwl:hasOBONamespace>GAZ</oboInOwl:hasOBONamespace>
        <oboInOwl:id>GAZ:00057301</oboInOwl:id>
        <rdfs:label>Volcan Sosneado</rdfs:label>
    </owl:NamedIndividual>
    


    <!-- http://purl.obolibrary.org/obo/GAZ_00057302 -->

    <owl:NamedIndividual rdf:about="http://purl.obolibrary.org/obo/GAZ_00057302">
        <obo:RO_0001025 rdf:resource="http://purl.obolibrary.org/obo/GAZ_00056701"/>
        <obo:IAO_0000115>A stratovolcano.</obo:IAO_0000115>
        <oboInOwl:hasOBONamespace>GAZ</oboInOwl:hasOBONamespace>
        <oboInOwl:id>GAZ:00057302</oboInOwl:id>
        <rdfs:label>Cerro Frey Carlos</rdfs:label>
    </owl:NamedIndividual>
    


    <!-- http://purl.obolibrary.org/obo/GAZ_00057303 -->

    <owl:NamedIndividual rdf:about="http://purl.obolibrary.org/obo/GAZ_00057303">
        <obo:RO_0001025 rdf:resource="http://purl.obolibrary.org/obo/GAZ_00056668"/>
        <obo:IAO_0000115>A volcanic cone.</obo:IAO_0000115>
        <oboInOwl:hasOBONamespace>GAZ</oboInOwl:hasOBONamespace>
        <oboInOwl:id>GAZ:00057303</oboInOwl:id>
        <rdfs:label>Volcan Peteroa</rdfs:label>
    </owl:NamedIndividual>
    


    <!-- http://purl.obolibrary.org/obo/GAZ_00057304 -->

    <owl:NamedIndividual rdf:about="http://purl.obolibrary.org/obo/GAZ_00057304">
        <obo:RO_0001025 rdf:resource="http://purl.obolibrary.org/obo/GAZ_00056668"/>
        <obo:IAO_0000115>A volcano.</obo:IAO_0000115>
        <oboInOwl:hasOBONamespace>GAZ</oboInOwl:hasOBONamespace>
        <oboInOwl:id>GAZ:00057304</oboInOwl:id>
        <rdfs:label>Volcan Planchon II</rdfs:label>
    </owl:NamedIndividual>
    


    <!-- http://purl.obolibrary.org/obo/GAZ_00057305 -->

    <owl:NamedIndividual rdf:about="http://purl.obolibrary.org/obo/GAZ_00057305">
        <obo:RO_0001025 rdf:resource="http://purl.obolibrary.org/obo/GAZ_00136453"/>
        <obo:IAO_0000115>A 26 x 14 km composite late-Pleistocene caldera that produced major rhyodacitic-to-dacitic ashflow sheets of ~200-500 cu km magma each, collectively referred to as the Loma Seca Tuff, at 0.8, 0.3, and 0.15 million years ago. Eruptive activity has continued into the Holocene, forming the 20-25 cu km dacitic-to-andesitic Cerro del Medio complex at the southern end of the caldera and the four clustered vents of Descabezado Chico near the western caldera rim. The late-Holocene 2.5 cu km Escorias dacitic lava flow from Descabezado Chico traveled &gt;30 km to the south. Several hot-spring clusters are present along the margin of the central resurgent uplift within the caldera.</obo:IAO_0000115>
        <oboInOwl:hasOBONamespace>GAZ</oboInOwl:hasOBONamespace>
        <oboInOwl:id>GAZ:00057305</oboInOwl:id>
        <rdfs:label>Calabozos Caldera</rdfs:label>
    </owl:NamedIndividual>
    


    <!-- http://purl.obolibrary.org/obo/GAZ_00057306 -->

    <owl:NamedIndividual rdf:about="http://purl.obolibrary.org/obo/GAZ_00057306">
        <obo:RO_0001025 rdf:resource="http://purl.obolibrary.org/obo/GAZ_00136453"/>
        <obo:IAO_0000115>A 15 x 25 km wide caldera that contains a cluster of small stratovolcanoes, lava domes, and pyroclastic cones of Pleistocene-to-Holocene age. The caldera lies mostly on the Chilean side of the border, but partially extends into Argentina. Fourteen Pleistocene basaltic lava flows were erupted down the upper part of the Maule river valley. A cluster of Pleistocene cinder cones was constructed on the NW side of the Maule lake, which occupies part of the northern portion of the caldera. The latest activity produced an explosion crater on the east side of the lake and a series of Holocene rhyolitic lava domes and blocky lava flows that surround Laguna del Maule.</obo:IAO_0000115>
        <oboInOwl:hasOBONamespace>GAZ</oboInOwl:hasOBONamespace>
        <oboInOwl:id>GAZ:00057306</oboInOwl:id>
        <rdfs:label>Laguna del Maule Caldera</rdfs:label>
    </owl:NamedIndividual>
    


    <!-- http://purl.obolibrary.org/obo/GAZ_00057307 -->

    <owl:NamedIndividual rdf:about="http://purl.obolibrary.org/obo/GAZ_00057307">
        <obo:RO_0001025 rdf:resource="http://purl.obolibrary.org/obo/GAZ_00057306"/>
        <obo:IAO_0000115>A freshwater caldera lake.</obo:IAO_0000115>
        <oboInOwl:hasOBONamespace>GAZ</oboInOwl:hasOBONamespace>
        <oboInOwl:id>GAZ:00057307</oboInOwl:id>
        <rdfs:label>Laguna del Maule</rdfs:label>
    </owl:NamedIndividual>
    


    <!-- http://purl.obolibrary.org/obo/GAZ_00057308 -->

    <owl:NamedIndividual rdf:about="http://purl.obolibrary.org/obo/GAZ_00057308">
        <obo:RO_0001025 rdf:resource="http://purl.obolibrary.org/obo/GAZ_00136453"/>
        <obo:IAO_0000115>A volcanic complex thathas been active from the Pliocene to the Holocene. The Tatara-San Pedro edifice overlies the deeply eroded Pellado stratovolcano; both were constructed within the 6 x 12 km Rio Colorado caldera, which formed during an eruption about 0.5 million years ago. The Tatara basaltic-andesite shield volcano at the western end of the complex contains stacked sequences of up to 100 or more lava flows forming up to 1500 m of relief. The glacier-filled summit crater of the 3621 m high dominantly andesitic San Pedro stratovolcano, which overlies the Tatara edifice, contains a young scoria cone that was the site of the most recent eruptions from the volcano. A major Holocene east-flank debris avalanche filled the Rio de la Puente valley to the south and was followed by eruptions originating within the avalanche scarp low on the east flank that produced lava flows down the Estero Pellado drainage. No historical eruptions have been recorded, but fumaroles are found SE of Pellado.</obo:IAO_0000115>
        <oboInOwl:hasOBONamespace>GAZ</oboInOwl:hasOBONamespace>
        <oboInOwl:id>GAZ:00057308</oboInOwl:id>
        <rdfs:label>San Pedro-Pellado Volcanic Complex</rdfs:label>
    </owl:NamedIndividual>
    


    <!-- http://purl.obolibrary.org/obo/GAZ_00057309 -->

    <owl:NamedIndividual rdf:about="http://purl.obolibrary.org/obo/GAZ_00057309">
        <obo:RO_0001025 rdf:resource="http://purl.obolibrary.org/obo/GAZ_00136453"/>
        <obo:IAO_0000115>A small shield-like stratovolcano of late-Pleistocene to Holocene age (Moreno and Naranjo, 1991) located about 15 km SE of Nevado de Longavi volcano. A 2.3 km wide caldera, possibly formed by edifice collapse, is open to the SE. Basaltic-andesite aa lava flows extend 7 km from the collapse scarp. The basaltic central cone rises about 500 m to an elevation of 2268 m. Much of the volcano is covered by pumice deposits that probably originated from Nevado de Longavi.</obo:IAO_0000115>
        <oboInOwl:hasOBONamespace>GAZ</oboInOwl:hasOBONamespace>
        <oboInOwl:id>GAZ:00057309</oboInOwl:id>
        <rdfs:label>Volcan Lomas Blancas</rdfs:label>
    </owl:NamedIndividual>
    


    <!-- http://purl.obolibrary.org/obo/GAZ_00057310 -->

    <owl:NamedIndividual rdf:about="http://purl.obolibrary.org/obo/GAZ_00057310">
        <obo:RO_0001025 rdf:resource="http://purl.obolibrary.org/obo/GAZ_00136453"/>
        <obo:IAO_0000115>A cinder cone with a double crater. It produced a basaltic-andesite lava flow that traveled about 3 km to the WNW into Laguna Dial.</obo:IAO_0000115>
        <oboInOwl:hasOBONamespace>GAZ</oboInOwl:hasOBONamespace>
        <oboInOwl:id>GAZ:00057310</oboInOwl:id>
        <rdfs:label>Volcan Resago</rdfs:label>
    </owl:NamedIndividual>
    


    <!-- http://purl.obolibrary.org/obo/GAZ_00057311 -->

    <owl:NamedIndividual rdf:about="http://purl.obolibrary.org/obo/GAZ_00057311">
        <obo:RO_0001025 rdf:resource="http://purl.obolibrary.org/obo/GAZ_00136453"/>
        <obo:IAO_0000115>A minor volcanic center that lies SSE of Copahue volcano and ENE of Tolguaca volcano. It consists of two craters of Holocene age (Gonzalez-Ferran, 1995) 2 km apart along a NE-trending fault that produced andesitic pyroclastic material and lava flows with columnar jointing. Cerro Chapulul is a 2143 m high Holocene cinder cone in this area of the Malleco province of central Chile. The cone occupies a plateau ranging from 2000-2300 m in altitude.</obo:IAO_0000115>
        <oboInOwl:hasOBONamespace>GAZ</oboInOwl:hasOBONamespace>
        <oboInOwl:id>GAZ:00057311</oboInOwl:id>
        <rdfs:label>Volcan Laguna Marinaqui</rdfs:label>
    </owl:NamedIndividual>
    


    <!-- http://purl.obolibrary.org/obo/GAZ_00057312 -->

    <owl:NamedIndividual rdf:about="http://purl.obolibrary.org/obo/GAZ_00057312">
        <obo:RO_0001025 rdf:resource="http://purl.obolibrary.org/obo/GAZ_00136453"/>
        <obo:IAO_0000115>A late-Pleistocene to Holocene stratovolcano located immediately NW of Lonquimay volcano. Only fumarolic activity has occurred from basaltic-andesitic Tolguaca during historical time. A NW-SE zone of aligned summit craters is youngest to the NW. Another group of vents cutting the south and east flanks is oriented SW-NE, parallel to the zone of flank vents on nearby Lonquimay volcano, and is of postglacial age (Moreno and Gardeweg 1989).</obo:IAO_0000115>
        <oboInOwl:hasOBONamespace>GAZ</oboInOwl:hasOBONamespace>
        <oboInOwl:id>GAZ:00057312</oboInOwl:id>
        <rdfs:label>Volcan Tolguaca</rdfs:label>
    </owl:NamedIndividual>
    


    <!-- http://purl.obolibrary.org/obo/GAZ_00057313 -->

    <owl:NamedIndividual rdf:about="http://purl.obolibrary.org/obo/GAZ_00057313">
        <obo:RO_0001025 rdf:resource="http://purl.obolibrary.org/obo/GAZ_00136453"/>
        <obo:IAO_0000115>A 4 km wide, glacier-filled caldera that lies to the east of the Pleistocene Nevados de Sollipulli complex. Major silicic pyroclastic rocks associated with caldera formation have not been found, and the caldera may have a non-explosive origin. Post-caldera eruptions have been focused along the caldera walls and have increased its height. A series of dacitic lava domes lines the eastern and southern caldera rims. The 1 km wide Alpehue crater, which cuts the SW rim, was the source of a large plinian eruption 2900 years before present (BP). Explosion craters and scoria cones are found on the outer flanks of the caldera. Two north-flank cones produced lava flows during the latest documented activity about 700 years BP (Naranjo et al., 1993). This low-profile volcano is less prominent than its neighbors Llaima and Villarrica, but its explosive history makes it a potentially hazardous volcanic center.</obo:IAO_0000115>
        <oboInOwl:hasOBONamespace>GAZ</oboInOwl:hasOBONamespace>
        <oboInOwl:id>GAZ:00057313</oboInOwl:id>
        <rdfs:label>Sollipulli Caldera</rdfs:label>
    </owl:NamedIndividual>
    


    <!-- http://purl.obolibrary.org/obo/GAZ_00057498 -->

    <owl:NamedIndividual rdf:about="http://purl.obolibrary.org/obo/GAZ_00057498">
        <obo:RO_0001025 rdf:resource="http://purl.obolibrary.org/obo/GAZ_00004639"/>
        <obo:RO_0001025 rdf:resource="http://purl.obolibrary.org/obo/GAZ_00136453"/>
        <obo:IAO_0000115>A volcanic field that consists of about 20 basaltic maars and cinder cones of Holocene age on a NNE-SSW alignment. The volcanic field occupies a low-lying area between the southern end of Ensenada Cayutue, the southern extension of Lake Todos los Santos, and the northern end of the Estuario Reloncavi, where the Rio Petrohue, which drains lake Todos los Santos, reaches the sea. The volcanic field lies along the major regional N-S-trending Liquine-Ofqui fault zone. La Vigueria and Volcan Cayutue are the principal cones. Formation of La Vigueria cone and associated lava flows temporarily dammed the Rio Petrohue about 3000 years ago, forming an ephemeral lake that was filled with deposits from Calbuco and Osorno volcanoes. Pyroclastic cones and lava flows of Volcen Cayutue filled the Ensenada de Cayutue depression, separating Lake Todos los Santos from Ralun Bay.</obo:IAO_0000115>
        <oboInOwl:hasOBONamespace>GAZ</oboInOwl:hasOBONamespace>
        <oboInOwl:id>GAZ:00057498</oboInOwl:id>
        <rdfs:label>Cayutue-La Vigueria Volcanic Field</rdfs:label>
    </owl:NamedIndividual>
    


    <!-- http://purl.obolibrary.org/obo/GAZ_00057499 -->

    <owl:NamedIndividual rdf:about="http://purl.obolibrary.org/obo/GAZ_00057499">
        <obo:RO_0001025 rdf:resource="http://purl.obolibrary.org/obo/GAZ_00136453"/>
        <obo:IAO_0000115>A 1862 m high partially glacially eroded basaltic stratovolcano. Numerous satellitic pyroclastic cones and associated basaltic lava flows were formed during the Holocene, principally on the SW flank and from the summit to the NW base of the volcano.</obo:IAO_0000115>
        <oboInOwl:hasOBONamespace>GAZ</oboInOwl:hasOBONamespace>
        <oboInOwl:id>GAZ:00057499</oboInOwl:id>
        <rdfs:label>Cuernos del Diablo</rdfs:label>
    </owl:NamedIndividual>
    


    <!-- http://purl.obolibrary.org/obo/GAZ_00057500 -->

    <owl:NamedIndividual rdf:about="http://purl.obolibrary.org/obo/GAZ_00057500">
        <obo:RO_0001025 rdf:resource="http://purl.obolibrary.org/obo/GAZ_00136453"/>
        <obo:IAO_0000115>A volcanic field in the northern Patagonia region of Argentina that covers an area of about 700 km2. The volcanic field lies about 400 km east of the Peru-Chile trench along the broad regional, NW-SE-trending Gastre fault system. Nine cinder cones and spatter cones produced blocky lava flows of alkali basaltic, basanitic, and trachybasaltic composition. One of the largest features of the volcanic field is Cerro Fermin, a cinder cone that produced a half dozen lava flows. The highest cone, 1359-m Cerro Negro, fed lava flows that traveled to the west, east, and then NE, where its distal margin is cut by a provincial road. Some of the lava flows, such as those from Cerro Ventana and Cerro Contreras, cover Holocene shorelines of playa lakes.</obo:IAO_0000115>
        <oboInOwl:hasOBONamespace>GAZ</oboInOwl:hasOBONamespace>
        <oboInOwl:id>GAZ:00057500</oboInOwl:id>
        <rdfs:label>Crater Basalt Volcanic Field</rdfs:label>
    </owl:NamedIndividual>
    


    <!-- http://purl.obolibrary.org/obo/GAZ_00057501 -->

    <owl:NamedIndividual rdf:about="http://purl.obolibrary.org/obo/GAZ_00057501">
        <obo:RO_0001025 rdf:resource="http://purl.obolibrary.org/obo/GAZ_00136453"/>
        <obo:IAO_0000115>A small, glacier-free volcano in the center of the Huequi Peninsula in the Gulf of Ancud. A parasitic cone is located on the west side of the 1318 m high basaltic-andesite volcano, which has an 800-m-wide crater. Explosive eruptions were recorded during the 19th and 20th centuries, initially in 1890 and most recently in about 1920.</obo:IAO_0000115>
        <oboInOwl:hasOBONamespace>GAZ</oboInOwl:hasOBONamespace>
        <oboInOwl:id>GAZ:00057501</oboInOwl:id>
        <rdfs:label>Volcan Huequi</rdfs:label>
    </owl:NamedIndividual>
    


    <!-- http://purl.obolibrary.org/obo/GAZ_00057503 -->

    <owl:NamedIndividual rdf:about="http://purl.obolibrary.org/obo/GAZ_00057503">
        <obo:RO_0001025 rdf:resource="http://purl.obolibrary.org/obo/GAZ_00136453"/>
        <obo:IAO_0000115>A volcano group that consists of five cinder cones oriented along a NNE trend NE of Melimoyu volcano.</obo:IAO_0000115>
        <oboInOwl:hasOBONamespace>GAZ</oboInOwl:hasOBONamespace>
        <oboInOwl:id>GAZ:00057503</oboInOwl:id>
        <rdfs:label>Palena Volcanic Group</rdfs:label>
    </owl:NamedIndividual>
    


    <!-- http://purl.obolibrary.org/obo/GAZ_00057504 -->

    <owl:NamedIndividual rdf:about="http://purl.obolibrary.org/obo/GAZ_00057504">
        <obo:RO_0001025 rdf:resource="http://purl.obolibrary.org/obo/GAZ_00136453"/>
        <obo:IAO_0000115>A stratovolcano located east of Maca volcano and NW of the town of Puerto Aisen, is a basaltic and dacitic stratovolcano. An explosion crater is open to the east, and about a half dozen explosion craters and pyroclastic cones lie along a fissure trending SW of the summit. Another 10 basaltic pyroclastic cones are located along second parallel fissure 5 km to the SE that is part of the major regional Liquine-Ofqui fault zone.</obo:IAO_0000115>
        <oboInOwl:hasOBONamespace>GAZ</oboInOwl:hasOBONamespace>
        <oboInOwl:id>GAZ:00057504</oboInOwl:id>
        <rdfs:label>Volcan Cay</rdfs:label>
    </owl:NamedIndividual>
    


    <!-- http://purl.obolibrary.org/obo/GAZ_00057505 -->

    <owl:NamedIndividual rdf:about="http://purl.obolibrary.org/obo/GAZ_00057505">
        <obo:RO_0001025 rdf:resource="http://purl.obolibrary.org/obo/GAZ_00136453"/>
        <obo:IAO_0000115>Basaltic lava flows that were emplaced on valley floors along the Rio Murta, about 30 km SE of Hudson volcano. The river follows a glacially carved valley cut into granitic rocks of the North Patagonian Batholith. The columnar-jointed lava flows include pillow lavas, lava tubes, and subglacial and sublacustral deposits. They have been considered to be of Holocene age due to lack of erosion and only locally subglacial emplacement.</obo:IAO_0000115>
        <oboInOwl:hasOBONamespace>GAZ</oboInOwl:hasOBONamespace>
        <oboInOwl:id>GAZ:00057505</oboInOwl:id>
        <rdfs:label>Rio Murta Cones</rdfs:label>
    </owl:NamedIndividual>
    


    <!-- http://purl.obolibrary.org/obo/GAZ_00057506 -->

    <owl:NamedIndividual rdf:about="http://purl.obolibrary.org/obo/GAZ_00057506">
        <obo:RO_0001025 rdf:resource="http://purl.obolibrary.org/obo/GAZ_00136454"/>
        <obo:IAO_0000115>A 1000 m high volcano (cinder cone) that consists of a large dacitic pyroclastic cone with a crater about 1 km in diameter. As many as a half dozen tephra layers overlie a peat layer dated at 3780 years before present. The volcano is being actively eroded by the Amalia Glacier, which drains off the Patagonian Icecap. Later work revealed evidence for historical eruptions in the 19th and early 20th centuries.</obo:IAO_0000115>
        <oboInOwl:hasOBONamespace>GAZ</oboInOwl:hasOBONamespace>
        <oboInOwl:id>GAZ:00057506</oboInOwl:id>
        <rdfs:label>Volcan Reclus</rdfs:label>
    </owl:NamedIndividual>
    


    <!-- http://purl.obolibrary.org/obo/GAZ_00057507 -->

    <owl:NamedIndividual rdf:about="http://purl.obolibrary.org/obo/GAZ_00057507">
        <obo:RO_0001025 rdf:resource="http://purl.obolibrary.org/obo/GAZ_00136454"/>
        <obo:IAO_0000115>A group of andesitic, columnar-jointed lava domes and pyroclastic cones up to 150 m high on Isla Cook mark the southernmost Holocene volcanoes of the Andes. The nearest Holocene volcanism occurs 400 km NW, at Monte Burney. The volcanoes, known as Volcan Cook or Volcan Fueguino, occupy a broad peninsula forming the SE end of Isla Cook. One of the cones, south of Bahia del Volcan, contains a 150-m-wide crater with a small lake. The lava domes and pyroclastic cones, possibly emplaced along N-S-trending faults, are unaffected by glacial erosion that scoured the underlying plutonic rocks. Passing navigators observed possible eruptive activity in the direction of Cook in 1712 and the eruption of incandescent ejecta in 1820.</obo:IAO_0000115>
        <oboInOwl:hasOBONamespace>GAZ</oboInOwl:hasOBONamespace>
        <oboInOwl:id>GAZ:00057507</oboInOwl:id>
        <rdfs:label>Volcan Fueguino</rdfs:label>
    </owl:NamedIndividual>
    


    <!-- http://purl.obolibrary.org/obo/GAZ_00057706 -->

    <owl:NamedIndividual rdf:about="http://purl.obolibrary.org/obo/GAZ_00057706">
        <obo:RO_0001025 rdf:resource="http://purl.obolibrary.org/obo/GAZ_00002931"/>
        <obo:IAO_0000115>A desert located in the northernmost part of Colombia in the La Guajira Department, covering most of La Guajira Peninsula including Venezuelan territory.</obo:IAO_0000115>
        <oboInOwl:hasOBONamespace>GAZ</oboInOwl:hasOBONamespace>
        <oboInOwl:id>GAZ:00057706</oboInOwl:id>
        <rdfs:label>La Guajira Desert</rdfs:label>
    </owl:NamedIndividual>
    


    <!-- http://purl.obolibrary.org/obo/GAZ_00057707 -->

    <owl:NamedIndividual rdf:about="http://purl.obolibrary.org/obo/GAZ_00057707">
        <obo:RO_0001025 rdf:resource="http://purl.obolibrary.org/obo/GAZ_00057708"/>
        <obo:IAO_0000115>A national park located in the State of Falcon, near the city of Coro on the road that leads to Paraguana. The Medanos park lies on the Isthmus of Medanos. A desert area, the massive sand dunes, known as Medanos, spread over an area of approximately 5 by 30 kms. They can reach 40 meters in height and are constantly transformed by the unrelenting wind.</obo:IAO_0000115>
        <oboInOwl:hasOBONamespace>GAZ</oboInOwl:hasOBONamespace>
        <oboInOwl:id>GAZ:00057707</oboInOwl:id>
        <rdfs:label>Medanos de Coro National Park</rdfs:label>
    </owl:NamedIndividual>
    


    <!-- http://purl.obolibrary.org/obo/GAZ_00057708 -->

    <owl:NamedIndividual rdf:about="http://purl.obolibrary.org/obo/GAZ_00057708">
        <obo:RO_0001025 rdf:resource="http://purl.obolibrary.org/obo/GAZ_00011614"/>
        <oboInOwl:hasOBONamespace>GAZ</oboInOwl:hasOBONamespace>
        <oboInOwl:id>GAZ:00057708</oboInOwl:id>
        <rdfs:label>Isthmus of Medanos</rdfs:label>
    </owl:NamedIndividual>
    


    <!-- http://purl.obolibrary.org/obo/GAZ_00058585 -->

    <owl:NamedIndividual rdf:about="http://purl.obolibrary.org/obo/GAZ_00058585">
        <obo:IAO_0000115>A glacier fed lake located on the eastern edge of the southern Andes, straddling the border between Argentina and Chile. The border is a peninsula the juts out into the lake on the North side. The border to the North of the lake follows the ridgeline of the last major expression of the eastern Andes.</obo:IAO_0000115>
        <oboInOwl:hasOBONamespace>GAZ</oboInOwl:hasOBONamespace>
        <oboInOwl:id>GAZ:00058585</oboInOwl:id>
        <rdfs:label>Lago Cochrane</rdfs:label>
    </owl:NamedIndividual>
    


    <!-- http://purl.obolibrary.org/obo/GAZ_00058772 -->

    <owl:NamedIndividual rdf:about="http://purl.obolibrary.org/obo/GAZ_00058772">
        <obo:RO_0001025 rdf:resource="http://purl.obolibrary.org/obo/GAZ_00056265"/>
        <obo:IAO_0000115>Valleys enclosed between the parallel mountain ranges of the Cordillera de la Costa.</obo:IAO_0000115>
        <oboInOwl:hasOBONamespace>GAZ</oboInOwl:hasOBONamespace>
        <oboInOwl:id>GAZ:00058772</oboInOwl:id>
        <rdfs:label>Aragua Valleys</rdfs:label>
    </owl:NamedIndividual>
    


    <!-- http://purl.obolibrary.org/obo/GAZ_00058773 -->

    <owl:NamedIndividual rdf:about="http://purl.obolibrary.org/obo/GAZ_00058773">
        <obo:RO_0001025 rdf:resource="http://purl.obolibrary.org/obo/GAZ_00002931"/>
        <obo:RO_0001025 rdf:resource="http://purl.obolibrary.org/obo/GAZ_00058772"/>
        <obo:IAO_0000115>An endorheic lake that occupies one of the Aragua Valleys, enclosed between the parallel mountain ranges of the Cordillera de la Costa, the Maritime Andes.</obo:IAO_0000115>
        <oboInOwl:hasOBONamespace>GAZ</oboInOwl:hasOBONamespace>
        <oboInOwl:id>GAZ:00058773</oboInOwl:id>
        <rdfs:label>Lago de Valencia</rdfs:label>
    </owl:NamedIndividual>
    


    <!-- http://purl.obolibrary.org/obo/GAZ_00062306 -->

    <owl:NamedIndividual rdf:about="http://purl.obolibrary.org/obo/GAZ_00062306">
        <obo:RO_0001025 rdf:resource="http://purl.obolibrary.org/obo/GAZ_00089671"/>
        <obo:IAO_0000115>A small lake of glacial origin in the Nevados National Park, in the Risaralda department of Colombia. It is fed by meltwaters from the Nevado Santa Isabel. Laguna del Otun is the source of the Otun River.</obo:IAO_0000115>
        <oboInOwl:hasOBONamespace>GAZ</oboInOwl:hasOBONamespace>
        <oboInOwl:id>GAZ:00062306</oboInOwl:id>
        <rdfs:label>Laguna del Otun</rdfs:label>
    </owl:NamedIndividual>
    


    <!-- http://purl.obolibrary.org/obo/GAZ_00062307 -->

    <owl:NamedIndividual rdf:about="http://purl.obolibrary.org/obo/GAZ_00062307">
        <obo:IAO_0000115>A freshwater Andean lake in Colombia, located in the east of Boyaca.</obo:IAO_0000115>
        <oboInOwl:hasOBONamespace>GAZ</oboInOwl:hasOBONamespace>
        <oboInOwl:id>GAZ:00062307</oboInOwl:id>
        <rdfs:label>Laguna de Tota</rdfs:label>
    </owl:NamedIndividual>
    


    <!-- http://purl.obolibrary.org/obo/GAZ_00062470 -->

    <owl:NamedIndividual rdf:about="http://purl.obolibrary.org/obo/GAZ_00062470">
        <obo:RO_0001025 rdf:resource="http://purl.obolibrary.org/obo/GAZ_00056605"/>
        <obo:IAO_0000115>A glacier lake in the Andes-Cordillera of South America in northwestern Peru.</obo:IAO_0000115>
        <oboInOwl:hasOBONamespace>GAZ</oboInOwl:hasOBONamespace>
        <oboInOwl:id>GAZ:00062470</oboInOwl:id>
        <rdfs:label>Laguna Palcacocha</rdfs:label>
    </owl:NamedIndividual>
    


    <!-- http://purl.obolibrary.org/obo/GAZ_00062471 -->

    <owl:NamedIndividual rdf:about="http://purl.obolibrary.org/obo/GAZ_00062471">
        <obo:RO_0001025 rdf:resource="http://purl.obolibrary.org/obo/GAZ_00146247"/>
        <obo:IAO_0000115>A lake in the Andes mountains of central Peru. It Is the northernmost of the lakes fed by the Andean glaciers, 20 km east of Cerro Yerupaja and 190 km NNE of the Peruvian capital Lima. The lake lies at an elevation of 3,845 m. Lago Lauricocha gets its water from small rivers coming down from the Cordillere Raura. The Rio Lauricocha issues from Lago Lauricocha and later joins Rio MaraNOn, which is one of the headwaters of the Amazon River.</obo:IAO_0000115>
        <oboInOwl:hasOBONamespace>GAZ</oboInOwl:hasOBONamespace>
        <oboInOwl:id>GAZ:00062471</oboInOwl:id>
        <rdfs:label>Lago Lauricocha</rdfs:label>
    </owl:NamedIndividual>
    


    <!-- http://purl.obolibrary.org/obo/GAZ_00062473 -->

    <owl:NamedIndividual rdf:about="http://purl.obolibrary.org/obo/GAZ_00062473">
        <obo:IAO_0000115>A lake in the Andes-Cordillera of South America in north-western Peru. It is located in the Ancash Region, on the road from Callejon de Huaylas to Chiquian. The lake is seen as the headwaters of Rio Santa which from here runs 200 km in a northerly direction, between Cordillera Negra and the snowcapped Cordillera Blanca.</obo:IAO_0000115>
        <oboInOwl:hasOBONamespace>GAZ</oboInOwl:hasOBONamespace>
        <oboInOwl:id>GAZ:00062473</oboInOwl:id>
        <rdfs:label>Laguna Conococha</rdfs:label>
    </owl:NamedIndividual>
    


    <!-- http://purl.obolibrary.org/obo/GAZ_00062577 -->

    <owl:NamedIndividual rdf:about="http://purl.obolibrary.org/obo/GAZ_00062577">
        <obo:IAO_0000115>A lake located east of Ranco Lake in the Andean mountains of southern Chile. The lake is of glacial origin and it is enclosed by mountain ranges of the Andes, by all sides, and drains west to Ranco Lake.</obo:IAO_0000115>
        <oboInOwl:hasOBONamespace>GAZ</oboInOwl:hasOBONamespace>
        <oboInOwl:id>GAZ:00062577</oboInOwl:id>
        <rdfs:label>Lago Maihue</rdfs:label>
    </owl:NamedIndividual>
    


    <!-- http://purl.obolibrary.org/obo/GAZ_00062584 -->

    <owl:NamedIndividual rdf:about="http://purl.obolibrary.org/obo/GAZ_00062584">
        <obo:IAO_0000115>A river that rises in the west Andes, flowing into the Pacific Ocean, crossing the Chilean city of La Serena.</obo:IAO_0000115>
        <oboInOwl:hasOBONamespace>GAZ</oboInOwl:hasOBONamespace>
        <oboInOwl:id>GAZ:00062584</oboInOwl:id>
        <rdfs:label>Rio Elqui</rdfs:label>
    </owl:NamedIndividual>
    


    <!-- http://purl.obolibrary.org/obo/GAZ_00062585 -->

    <owl:NamedIndividual rdf:about="http://purl.obolibrary.org/obo/GAZ_00062585">
        <obo:RO_0001025 rdf:resource="http://purl.obolibrary.org/obo/GAZ_00062584"/>
        <obo:IAO_0000115>An artificial lake created by a dam on the Elqui River, 60 km east of the city of La Serena.</obo:IAO_0000115>
        <oboInOwl:hasOBONamespace>GAZ</oboInOwl:hasOBONamespace>
        <oboInOwl:id>GAZ:00062585</oboInOwl:id>
        <rdfs:label>Tranque Puclaro</rdfs:label>
    </owl:NamedIndividual>
    


    <!-- http://purl.obolibrary.org/obo/GAZ_00062586 -->

    <owl:NamedIndividual rdf:about="http://purl.obolibrary.org/obo/GAZ_00062586">
        <obo:IAO_0000115>A saline lake in the Andes Mountains of Chile. It lies in the Atacama Region, near San Francisco Pass. The volcano Ojos del Salado marks the south border of its basin.</obo:IAO_0000115>
        <oboInOwl:hasOBONamespace>GAZ</oboInOwl:hasOBONamespace>
        <oboInOwl:id>GAZ:00062586</oboInOwl:id>
        <rdfs:label>Laguna Verde</rdfs:label>
    </owl:NamedIndividual>
    


    <!-- http://purl.obolibrary.org/obo/GAZ_00071532 -->

    <owl:NamedIndividual rdf:about="http://purl.obolibrary.org/obo/GAZ_00071532">
        <obo:RO_0001025 rdf:resource="http://purl.obolibrary.org/obo/GAZ_00011618"/>
        <oboInOwl:hasOBONamespace>GAZ</oboInOwl:hasOBONamespace>
        <oboInOwl:id>GAZ:00071532</oboInOwl:id>
        <rdfs:label>Municipality of Alto Orinoco</rdfs:label>
    </owl:NamedIndividual>
    


    <!-- http://purl.obolibrary.org/obo/GAZ_00071533 -->

    <owl:NamedIndividual rdf:about="http://purl.obolibrary.org/obo/GAZ_00071533">
        <obo:RO_0001025 rdf:resource="http://purl.obolibrary.org/obo/GAZ_00011618"/>
        <oboInOwl:hasOBONamespace>GAZ</oboInOwl:hasOBONamespace>
        <oboInOwl:id>GAZ:00071533</oboInOwl:id>
        <rdfs:label>Municipality of Manapiare</rdfs:label>
    </owl:NamedIndividual>
    


    <!-- http://purl.obolibrary.org/obo/GAZ_00071534 -->

    <owl:NamedIndividual rdf:about="http://purl.obolibrary.org/obo/GAZ_00071534">
        <obo:RO_0001025 rdf:resource="http://purl.obolibrary.org/obo/GAZ_00011618"/>
        <oboInOwl:hasOBONamespace>GAZ</oboInOwl:hasOBONamespace>
        <oboInOwl:id>GAZ:00071534</oboInOwl:id>
        <rdfs:label>Municipality of Rio Negro</rdfs:label>
    </owl:NamedIndividual>
    


    <!-- http://purl.obolibrary.org/obo/GAZ_00071535 -->

    <owl:NamedIndividual rdf:about="http://purl.obolibrary.org/obo/GAZ_00071535">
        <obo:RO_0001025 rdf:resource="http://purl.obolibrary.org/obo/GAZ_00011618"/>
        <oboInOwl:hasOBONamespace>GAZ</oboInOwl:hasOBONamespace>
        <oboInOwl:id>GAZ:00071535</oboInOwl:id>
        <rdfs:label>Municipality of Atures</rdfs:label>
    </owl:NamedIndividual>
    


    <!-- http://purl.obolibrary.org/obo/GAZ_00071536 -->

    <owl:NamedIndividual rdf:about="http://purl.obolibrary.org/obo/GAZ_00071536">
        <obo:RO_0001025 rdf:resource="http://purl.obolibrary.org/obo/GAZ_00011618"/>
        <oboInOwl:hasOBONamespace>GAZ</oboInOwl:hasOBONamespace>
        <oboInOwl:id>GAZ:00071536</oboInOwl:id>
        <rdfs:label>Municipality of Atabapo</rdfs:label>
    </owl:NamedIndividual>
    


    <!-- http://purl.obolibrary.org/obo/GAZ_00071537 -->

    <owl:NamedIndividual rdf:about="http://purl.obolibrary.org/obo/GAZ_00071537">
        <obo:RO_0001025 rdf:resource="http://purl.obolibrary.org/obo/GAZ_00011618"/>
        <oboInOwl:hasOBONamespace>GAZ</oboInOwl:hasOBONamespace>
        <oboInOwl:id>GAZ:00071537</oboInOwl:id>
        <rdfs:label>Municipality of Autana</rdfs:label>
    </owl:NamedIndividual>
    


    <!-- http://purl.obolibrary.org/obo/GAZ_00071538 -->

    <owl:NamedIndividual rdf:about="http://purl.obolibrary.org/obo/GAZ_00071538">
        <obo:RO_0001025 rdf:resource="http://purl.obolibrary.org/obo/GAZ_00011618"/>
        <oboInOwl:hasOBONamespace>GAZ</oboInOwl:hasOBONamespace>
        <oboInOwl:id>GAZ:00071538</oboInOwl:id>
        <rdfs:label>Municipality of Maroa</rdfs:label>
    </owl:NamedIndividual>
    


    <!-- http://purl.obolibrary.org/obo/GAZ_00071539 -->

    <owl:NamedIndividual rdf:about="http://purl.obolibrary.org/obo/GAZ_00071539">
        <obo:RO_0001025 rdf:resource="http://purl.obolibrary.org/obo/GAZ_00011587"/>
        <oboInOwl:hasOBONamespace>GAZ</oboInOwl:hasOBONamespace>
        <oboInOwl:id>GAZ:00071539</oboInOwl:id>
        <rdfs:label>Municipality of Francisco Linares Alcantara</rdfs:label>
    </owl:NamedIndividual>
    


    <!-- http://purl.obolibrary.org/obo/GAZ_00071540 -->

    <owl:NamedIndividual rdf:about="http://purl.obolibrary.org/obo/GAZ_00071540">
        <obo:RO_0001025 rdf:resource="http://purl.obolibrary.org/obo/GAZ_00011587"/>
        <oboInOwl:hasOBONamespace>GAZ</oboInOwl:hasOBONamespace>
        <oboInOwl:id>GAZ:00071540</oboInOwl:id>
        <rdfs:label>Municipality of Ocumare de la Costa de Oro</rdfs:label>
    </owl:NamedIndividual>
    


    <!-- http://purl.obolibrary.org/obo/GAZ_00071541 -->

    <owl:NamedIndividual rdf:about="http://purl.obolibrary.org/obo/GAZ_00071541">
        <obo:RO_0001025 rdf:resource="http://purl.obolibrary.org/obo/GAZ_00011587"/>
        <oboInOwl:hasOBONamespace>GAZ</oboInOwl:hasOBONamespace>
        <oboInOwl:id>GAZ:00071541</oboInOwl:id>
        <rdfs:label>Municipality of Zamora</rdfs:label>
    </owl:NamedIndividual>
    


    <!-- http://purl.obolibrary.org/obo/GAZ_00071542 -->

    <owl:NamedIndividual rdf:about="http://purl.obolibrary.org/obo/GAZ_00071542">
        <obo:RO_0001025 rdf:resource="http://purl.obolibrary.org/obo/GAZ_00011587"/>
        <oboInOwl:hasOBONamespace>GAZ</oboInOwl:hasOBONamespace>
        <oboInOwl:id>GAZ:00071542</oboInOwl:id>
        <rdfs:label>Municipality of San Casimiro</rdfs:label>
    </owl:NamedIndividual>
    


    <!-- http://purl.obolibrary.org/obo/GAZ_00071543 -->

    <owl:NamedIndividual rdf:about="http://purl.obolibrary.org/obo/GAZ_00071543">
        <obo:RO_0001025 rdf:resource="http://purl.obolibrary.org/obo/GAZ_00011587"/>
        <oboInOwl:hasOBONamespace>GAZ</oboInOwl:hasOBONamespace>
        <oboInOwl:id>GAZ:00071543</oboInOwl:id>
        <rdfs:label>Municipality of Santos Michelena</rdfs:label>
    </owl:NamedIndividual>
    


    <!-- http://purl.obolibrary.org/obo/GAZ_00071544 -->

    <owl:NamedIndividual rdf:about="http://purl.obolibrary.org/obo/GAZ_00071544">
        <obo:RO_0001025 rdf:resource="http://purl.obolibrary.org/obo/GAZ_00011587"/>
        <oboInOwl:hasOBONamespace>GAZ</oboInOwl:hasOBONamespace>
        <oboInOwl:id>GAZ:00071544</oboInOwl:id>
        <rdfs:label>Municipality of San Sebastian</rdfs:label>
    </owl:NamedIndividual>
    


    <!-- http://purl.obolibrary.org/obo/GAZ_00071545 -->

    <owl:NamedIndividual rdf:about="http://purl.obolibrary.org/obo/GAZ_00071545">
        <obo:RO_0001025 rdf:resource="http://purl.obolibrary.org/obo/GAZ_00011587"/>
        <oboInOwl:hasOBONamespace>GAZ</oboInOwl:hasOBONamespace>
        <oboInOwl:id>GAZ:00071545</oboInOwl:id>
        <rdfs:label>Municipality of Tovar</rdfs:label>
    </owl:NamedIndividual>
    


    <!-- http://purl.obolibrary.org/obo/GAZ_00071546 -->

    <owl:NamedIndividual rdf:about="http://purl.obolibrary.org/obo/GAZ_00071546">
        <obo:RO_0001025 rdf:resource="http://purl.obolibrary.org/obo/GAZ_00011587"/>
        <oboInOwl:hasOBONamespace>GAZ</oboInOwl:hasOBONamespace>
        <oboInOwl:id>GAZ:00071546</oboInOwl:id>
        <rdfs:label>Municipality of Bolivar</rdfs:label>
    </owl:NamedIndividual>
    


    <!-- http://purl.obolibrary.org/obo/GAZ_00071547 -->

    <owl:NamedIndividual rdf:about="http://purl.obolibrary.org/obo/GAZ_00071547">
        <obo:RO_0001025 rdf:resource="http://purl.obolibrary.org/obo/GAZ_00011587"/>
        <oboInOwl:hasOBONamespace>GAZ</oboInOwl:hasOBONamespace>
        <oboInOwl:id>GAZ:00071547</oboInOwl:id>
        <rdfs:label>Municipality of Jose Angel Lamas</rdfs:label>
    </owl:NamedIndividual>
    


    <!-- http://purl.obolibrary.org/obo/GAZ_00071548 -->

    <owl:NamedIndividual rdf:about="http://purl.obolibrary.org/obo/GAZ_00071548">
        <obo:RO_0001025 rdf:resource="http://purl.obolibrary.org/obo/GAZ_00011587"/>
        <oboInOwl:hasOBONamespace>GAZ</oboInOwl:hasOBONamespace>
        <oboInOwl:id>GAZ:00071548</oboInOwl:id>
        <rdfs:label>Municipality of Jose Rafael Revenga</rdfs:label>
    </owl:NamedIndividual>
    


    <!-- http://purl.obolibrary.org/obo/GAZ_00071549 -->

    <owl:NamedIndividual rdf:about="http://purl.obolibrary.org/obo/GAZ_00071549">
        <obo:RO_0001025 rdf:resource="http://purl.obolibrary.org/obo/GAZ_00011587"/>
        <oboInOwl:hasOBONamespace>GAZ</oboInOwl:hasOBONamespace>
        <oboInOwl:id>GAZ:00071549</oboInOwl:id>
        <rdfs:label>Municipality of Sucre</rdfs:label>
    </owl:NamedIndividual>
    


    <!-- http://purl.obolibrary.org/obo/GAZ_00071550 -->

    <owl:NamedIndividual rdf:about="http://purl.obolibrary.org/obo/GAZ_00071550">
        <obo:RO_0001025 rdf:resource="http://purl.obolibrary.org/obo/GAZ_00011587"/>
        <oboInOwl:hasOBONamespace>GAZ</oboInOwl:hasOBONamespace>
        <oboInOwl:id>GAZ:00071550</oboInOwl:id>
        <rdfs:label>Municipality of Santiago Marino</rdfs:label>
    </owl:NamedIndividual>
    


    <!-- http://purl.obolibrary.org/obo/GAZ_00071551 -->

    <owl:NamedIndividual rdf:about="http://purl.obolibrary.org/obo/GAZ_00071551">
        <obo:RO_0001025 rdf:resource="http://purl.obolibrary.org/obo/GAZ_00011587"/>
        <oboInOwl:hasOBONamespace>GAZ</oboInOwl:hasOBONamespace>
        <oboInOwl:id>GAZ:00071551</oboInOwl:id>
        <rdfs:label>Municipality of Urdaneta</rdfs:label>
    </owl:NamedIndividual>
    


    <!-- http://purl.obolibrary.org/obo/GAZ_00071552 -->

    <owl:NamedIndividual rdf:about="http://purl.obolibrary.org/obo/GAZ_00071552">
        <obo:RO_0001025 rdf:resource="http://purl.obolibrary.org/obo/GAZ_00011587"/>
        <oboInOwl:hasOBONamespace>GAZ</oboInOwl:hasOBONamespace>
        <oboInOwl:id>GAZ:00071552</oboInOwl:id>
        <rdfs:label>Municipality of Camatagua</rdfs:label>
    </owl:NamedIndividual>
    


    <!-- http://purl.obolibrary.org/obo/GAZ_00071553 -->

    <owl:NamedIndividual rdf:about="http://purl.obolibrary.org/obo/GAZ_00071553">
        <obo:RO_0001025 rdf:resource="http://purl.obolibrary.org/obo/GAZ_00011587"/>
        <oboInOwl:hasOBONamespace>GAZ</oboInOwl:hasOBONamespace>
        <oboInOwl:id>GAZ:00071553</oboInOwl:id>
        <rdfs:label>Municipality of Libertador</rdfs:label>
    </owl:NamedIndividual>
    


    <!-- http://purl.obolibrary.org/obo/GAZ_00071554 -->

    <owl:NamedIndividual rdf:about="http://purl.obolibrary.org/obo/GAZ_00071554">
        <obo:RO_0001025 rdf:resource="http://purl.obolibrary.org/obo/GAZ_00011587"/>
        <oboInOwl:hasOBONamespace>GAZ</oboInOwl:hasOBONamespace>
        <oboInOwl:id>GAZ:00071554</oboInOwl:id>
        <rdfs:label>Municipality of Jose Felix Ribas</rdfs:label>
    </owl:NamedIndividual>
    


    <!-- http://purl.obolibrary.org/obo/GAZ_00071555 -->

    <owl:NamedIndividual rdf:about="http://purl.obolibrary.org/obo/GAZ_00071555">
        <obo:RO_0001025 rdf:resource="http://purl.obolibrary.org/obo/GAZ_00011587"/>
        <oboInOwl:hasOBONamespace>GAZ</oboInOwl:hasOBONamespace>
        <oboInOwl:id>GAZ:00071555</oboInOwl:id>
        <rdfs:label>Municipality of Mario Briceno Iragorry</rdfs:label>
    </owl:NamedIndividual>
    


    <!-- http://purl.obolibrary.org/obo/GAZ_00071556 -->

    <owl:NamedIndividual rdf:about="http://purl.obolibrary.org/obo/GAZ_00071556">
        <obo:RO_0001025 rdf:resource="http://purl.obolibrary.org/obo/GAZ_00011587"/>
        <oboInOwl:hasOBONamespace>GAZ</oboInOwl:hasOBONamespace>
        <oboInOwl:id>GAZ:00071556</oboInOwl:id>
        <rdfs:label>Municipality of Girardot</rdfs:label>
    </owl:NamedIndividual>
    


    <!-- http://purl.obolibrary.org/obo/GAZ_00071557 -->

    <owl:NamedIndividual rdf:about="http://purl.obolibrary.org/obo/GAZ_00071557">
        <obo:RO_0001025 rdf:resource="http://purl.obolibrary.org/obo/GAZ_00011588"/>
        <oboInOwl:hasOBONamespace>GAZ</oboInOwl:hasOBONamespace>
        <oboInOwl:id>GAZ:00071557</oboInOwl:id>
        <rdfs:label>Municipality of Alberto Arvelo Torrealba</rdfs:label>
    </owl:NamedIndividual>
    


    <!-- http://purl.obolibrary.org/obo/GAZ_00071558 -->

    <owl:NamedIndividual rdf:about="http://purl.obolibrary.org/obo/GAZ_00071558">
        <obo:RO_0001025 rdf:resource="http://purl.obolibrary.org/obo/GAZ_00011588"/>
        <oboInOwl:hasOBONamespace>GAZ</oboInOwl:hasOBONamespace>
        <oboInOwl:id>GAZ:00071558</oboInOwl:id>
        <rdfs:label>Municipality of Antonio Jose de Sucre</rdfs:label>
    </owl:NamedIndividual>
    


    <!-- http://purl.obolibrary.org/obo/GAZ_00071559 -->

    <owl:NamedIndividual rdf:about="http://purl.obolibrary.org/obo/GAZ_00071559">
        <obo:RO_0001025 rdf:resource="http://purl.obolibrary.org/obo/GAZ_00011588"/>
        <oboInOwl:hasOBONamespace>GAZ</oboInOwl:hasOBONamespace>
        <oboInOwl:id>GAZ:00071559</oboInOwl:id>
        <rdfs:label>Municipality of Barinas</rdfs:label>
    </owl:NamedIndividual>
    


    <!-- http://purl.obolibrary.org/obo/GAZ_00071560 -->

    <owl:NamedIndividual rdf:about="http://purl.obolibrary.org/obo/GAZ_00071560">
        <obo:RO_0001025 rdf:resource="http://purl.obolibrary.org/obo/GAZ_00011588"/>
        <oboInOwl:hasOBONamespace>GAZ</oboInOwl:hasOBONamespace>
        <oboInOwl:id>GAZ:00071560</oboInOwl:id>
        <rdfs:label>Municipality of Andres Eloy Blanco</rdfs:label>
    </owl:NamedIndividual>
    


    <!-- http://purl.obolibrary.org/obo/GAZ_00071561 -->

    <owl:NamedIndividual rdf:about="http://purl.obolibrary.org/obo/GAZ_00071561">
        <obo:RO_0001025 rdf:resource="http://purl.obolibrary.org/obo/GAZ_00011588"/>
        <oboInOwl:hasOBONamespace>GAZ</oboInOwl:hasOBONamespace>
        <oboInOwl:id>GAZ:00071561</oboInOwl:id>
        <rdfs:label>Municipality of Obispos</rdfs:label>
    </owl:NamedIndividual>
    


    <!-- http://purl.obolibrary.org/obo/GAZ_00071562 -->

    <owl:NamedIndividual rdf:about="http://purl.obolibrary.org/obo/GAZ_00071562">
        <obo:RO_0001025 rdf:resource="http://purl.obolibrary.org/obo/GAZ_00011588"/>
        <oboInOwl:hasOBONamespace>GAZ</oboInOwl:hasOBONamespace>
        <oboInOwl:id>GAZ:00071562</oboInOwl:id>
        <rdfs:label>Municipality of Sosa</rdfs:label>
    </owl:NamedIndividual>
    


    <!-- http://purl.obolibrary.org/obo/GAZ_00071563 -->

    <owl:NamedIndividual rdf:about="http://purl.obolibrary.org/obo/GAZ_00071563">
        <obo:RO_0001025 rdf:resource="http://purl.obolibrary.org/obo/GAZ_00011588"/>
        <oboInOwl:hasOBONamespace>GAZ</oboInOwl:hasOBONamespace>
        <oboInOwl:id>GAZ:00071563</oboInOwl:id>
        <rdfs:label>Municipality of Cruz Paredes</rdfs:label>
    </owl:NamedIndividual>
    


    <!-- http://purl.obolibrary.org/obo/GAZ_00071564 -->

    <owl:NamedIndividual rdf:about="http://purl.obolibrary.org/obo/GAZ_00071564">
        <obo:RO_0001025 rdf:resource="http://purl.obolibrary.org/obo/GAZ_00011588"/>
        <oboInOwl:hasOBONamespace>GAZ</oboInOwl:hasOBONamespace>
        <oboInOwl:id>GAZ:00071564</oboInOwl:id>
        <rdfs:label>Municipality of Rojas</rdfs:label>
    </owl:NamedIndividual>
    


    <!-- http://purl.obolibrary.org/obo/GAZ_00071565 -->

    <owl:NamedIndividual rdf:about="http://purl.obolibrary.org/obo/GAZ_00071565">
        <obo:RO_0001025 rdf:resource="http://purl.obolibrary.org/obo/GAZ_00011588"/>
        <oboInOwl:hasOBONamespace>GAZ</oboInOwl:hasOBONamespace>
        <oboInOwl:id>GAZ:00071565</oboInOwl:id>
        <rdfs:label>Municipality of Ezequiel Zamora</rdfs:label>
    </owl:NamedIndividual>
    


    <!-- http://purl.obolibrary.org/obo/GAZ_00071566 -->

    <owl:NamedIndividual rdf:about="http://purl.obolibrary.org/obo/GAZ_00071566">
        <obo:RO_0001025 rdf:resource="http://purl.obolibrary.org/obo/GAZ_00011588"/>
        <oboInOwl:hasOBONamespace>GAZ</oboInOwl:hasOBONamespace>
        <oboInOwl:id>GAZ:00071566</oboInOwl:id>
        <rdfs:label>Municipality of Pedraza</rdfs:label>
    </owl:NamedIndividual>
    


    <!-- http://purl.obolibrary.org/obo/GAZ_00071567 -->

    <owl:NamedIndividual rdf:about="http://purl.obolibrary.org/obo/GAZ_00071567">
        <obo:RO_0001025 rdf:resource="http://purl.obolibrary.org/obo/GAZ_00011588"/>
        <oboInOwl:hasOBONamespace>GAZ</oboInOwl:hasOBONamespace>
        <oboInOwl:id>GAZ:00071567</oboInOwl:id>
        <rdfs:label>Municipality of Bolivar</rdfs:label>
    </owl:NamedIndividual>
    


    <!-- http://purl.obolibrary.org/obo/GAZ_00071568 -->

    <owl:NamedIndividual rdf:about="http://purl.obolibrary.org/obo/GAZ_00071568">
        <obo:RO_0001025 rdf:resource="http://purl.obolibrary.org/obo/GAZ_00011615"/>
        <oboInOwl:hasOBONamespace>GAZ</oboInOwl:hasOBONamespace>
        <oboInOwl:id>GAZ:00071568</oboInOwl:id>
        <rdfs:label>Municipality of El Callao</rdfs:label>
    </owl:NamedIndividual>
    


    <!-- http://purl.obolibrary.org/obo/GAZ_00071569 -->

    <owl:NamedIndividual rdf:about="http://purl.obolibrary.org/obo/GAZ_00071569">
        <obo:RO_0001025 rdf:resource="http://purl.obolibrary.org/obo/GAZ_00011615"/>
        <oboInOwl:hasOBONamespace>GAZ</oboInOwl:hasOBONamespace>
        <oboInOwl:id>GAZ:00071569</oboInOwl:id>
        <rdfs:label>Municipality of Sucre</rdfs:label>
    </owl:NamedIndividual>
    


    <!-- http://purl.obolibrary.org/obo/GAZ_00071570 -->

    <owl:NamedIndividual rdf:about="http://purl.obolibrary.org/obo/GAZ_00071570">
        <obo:RO_0001025 rdf:resource="http://purl.obolibrary.org/obo/GAZ_00011615"/>
        <oboInOwl:hasOBONamespace>GAZ</oboInOwl:hasOBONamespace>
        <oboInOwl:id>GAZ:00071570</oboInOwl:id>
        <rdfs:label>Municipality of Caroni</rdfs:label>
    </owl:NamedIndividual>
    


    <!-- http://purl.obolibrary.org/obo/GAZ_00071571 -->

    <owl:NamedIndividual rdf:about="http://purl.obolibrary.org/obo/GAZ_00071571">
        <obo:RO_0001025 rdf:resource="http://purl.obolibrary.org/obo/GAZ_00011615"/>
        <oboInOwl:hasOBONamespace>GAZ</oboInOwl:hasOBONamespace>
        <oboInOwl:id>GAZ:00071571</oboInOwl:id>
        <rdfs:label>Municipality of Cedeno</rdfs:label>
    </owl:NamedIndividual>
    


    <!-- http://purl.obolibrary.org/obo/GAZ_00071572 -->

    <owl:NamedIndividual rdf:about="http://purl.obolibrary.org/obo/GAZ_00071572">
        <obo:RO_0001025 rdf:resource="http://purl.obolibrary.org/obo/GAZ_00011615"/>
        <oboInOwl:hasOBONamespace>GAZ</oboInOwl:hasOBONamespace>
        <oboInOwl:id>GAZ:00071572</oboInOwl:id>
        <rdfs:label>Padre Pedro Chien</rdfs:label>
    </owl:NamedIndividual>
    


    <!-- http://purl.obolibrary.org/obo/GAZ_00071573 -->

    <owl:NamedIndividual rdf:about="http://purl.obolibrary.org/obo/GAZ_00071573">
        <obo:RO_0001025 rdf:resource="http://purl.obolibrary.org/obo/GAZ_00011615"/>
        <oboInOwl:hasOBONamespace>GAZ</oboInOwl:hasOBONamespace>
        <oboInOwl:id>GAZ:00071573</oboInOwl:id>
        <rdfs:label>Municipality of Gran Sabana</rdfs:label>
    </owl:NamedIndividual>
    


    <!-- http://purl.obolibrary.org/obo/GAZ_00071574 -->

    <owl:NamedIndividual rdf:about="http://purl.obolibrary.org/obo/GAZ_00071574">
        <obo:RO_0001025 rdf:resource="http://purl.obolibrary.org/obo/GAZ_00011615"/>
        <oboInOwl:hasOBONamespace>GAZ</oboInOwl:hasOBONamespace>
        <oboInOwl:id>GAZ:00071574</oboInOwl:id>
        <rdfs:label>Municipality of Piar</rdfs:label>
    </owl:NamedIndividual>
    


    <!-- http://purl.obolibrary.org/obo/GAZ_00071575 -->

    <owl:NamedIndividual rdf:about="http://purl.obolibrary.org/obo/GAZ_00071575">
        <obo:RO_0001025 rdf:resource="http://purl.obolibrary.org/obo/GAZ_00011615"/>
        <oboInOwl:hasOBONamespace>GAZ</oboInOwl:hasOBONamespace>
        <oboInOwl:id>GAZ:00071575</oboInOwl:id>
        <rdfs:label>Municipality of Roscio</rdfs:label>
    </owl:NamedIndividual>
    


    <!-- http://purl.obolibrary.org/obo/GAZ_00071576 -->

    <owl:NamedIndividual rdf:about="http://purl.obolibrary.org/obo/GAZ_00071576">
        <obo:RO_0001025 rdf:resource="http://purl.obolibrary.org/obo/GAZ_00011615"/>
        <oboInOwl:hasOBONamespace>GAZ</oboInOwl:hasOBONamespace>
        <oboInOwl:id>GAZ:00071576</oboInOwl:id>
        <rdfs:label>Municipality of Sifontes</rdfs:label>
    </owl:NamedIndividual>
    


    <!-- http://purl.obolibrary.org/obo/GAZ_00071577 -->

    <owl:NamedIndividual rdf:about="http://purl.obolibrary.org/obo/GAZ_00071577">
        <obo:RO_0001025 rdf:resource="http://purl.obolibrary.org/obo/GAZ_00011615"/>
        <oboInOwl:hasOBONamespace>GAZ</oboInOwl:hasOBONamespace>
        <oboInOwl:id>GAZ:00071577</oboInOwl:id>
        <rdfs:label>Municipality of Heres</rdfs:label>
    </owl:NamedIndividual>
    


    <!-- http://purl.obolibrary.org/obo/GAZ_00071578 -->

    <owl:NamedIndividual rdf:about="http://purl.obolibrary.org/obo/GAZ_00071578">
        <obo:RO_0001025 rdf:resource="http://purl.obolibrary.org/obo/GAZ_00011615"/>
        <oboInOwl:hasOBONamespace>GAZ</oboInOwl:hasOBONamespace>
        <oboInOwl:id>GAZ:00071578</oboInOwl:id>
        <rdfs:label>Municipality of Raul Leoni</rdfs:label>
    </owl:NamedIndividual>
    


    <!-- http://purl.obolibrary.org/obo/GAZ_00071579 -->

    <owl:NamedIndividual rdf:about="http://purl.obolibrary.org/obo/GAZ_00071579">
        <obo:RO_0001025 rdf:resource="http://purl.obolibrary.org/obo/GAZ_00011616"/>
        <oboInOwl:hasOBONamespace>GAZ</oboInOwl:hasOBONamespace>
        <oboInOwl:id>GAZ:00071579</oboInOwl:id>
        <rdfs:label>Municipality of Bejuma</rdfs:label>
    </owl:NamedIndividual>
    


    <!-- http://purl.obolibrary.org/obo/GAZ_00071580 -->

    <owl:NamedIndividual rdf:about="http://purl.obolibrary.org/obo/GAZ_00071580">
        <obo:RO_0001025 rdf:resource="http://purl.obolibrary.org/obo/GAZ_00011616"/>
        <oboInOwl:hasOBONamespace>GAZ</oboInOwl:hasOBONamespace>
        <oboInOwl:id>GAZ:00071580</oboInOwl:id>
        <rdfs:label>Municipality of Diego Ibarra</rdfs:label>
    </owl:NamedIndividual>
    


    <!-- http://purl.obolibrary.org/obo/GAZ_00071581 -->

    <owl:NamedIndividual rdf:about="http://purl.obolibrary.org/obo/GAZ_00071581">
        <obo:RO_0001025 rdf:resource="http://purl.obolibrary.org/obo/GAZ_00011616"/>
        <oboInOwl:hasOBONamespace>GAZ</oboInOwl:hasOBONamespace>
        <oboInOwl:id>GAZ:00071581</oboInOwl:id>
        <rdfs:label>Municipality of Valencia</rdfs:label>
    </owl:NamedIndividual>
    


    <!-- http://purl.obolibrary.org/obo/GAZ_00071582 -->

    <owl:NamedIndividual rdf:about="http://purl.obolibrary.org/obo/GAZ_00071582">
        <obo:RO_0001025 rdf:resource="http://purl.obolibrary.org/obo/GAZ_00011616"/>
        <oboInOwl:hasOBONamespace>GAZ</oboInOwl:hasOBONamespace>
        <oboInOwl:id>GAZ:00071582</oboInOwl:id>
        <rdfs:label>Municipality of Los Guayos</rdfs:label>
    </owl:NamedIndividual>
    


    <!-- http://purl.obolibrary.org/obo/GAZ_00071583 -->

    <owl:NamedIndividual rdf:about="http://purl.obolibrary.org/obo/GAZ_00071583">
        <obo:RO_0001025 rdf:resource="http://purl.obolibrary.org/obo/GAZ_00011617"/>
        <oboInOwl:hasOBONamespace>GAZ</oboInOwl:hasOBONamespace>
        <oboInOwl:id>GAZ:00071583</oboInOwl:id>
        <rdfs:label>Municipality of Antonio Diaz</rdfs:label>
    </owl:NamedIndividual>
    


    <!-- http://purl.obolibrary.org/obo/GAZ_00071584 -->

    <owl:NamedIndividual rdf:about="http://purl.obolibrary.org/obo/GAZ_00071584">
        <obo:RO_0001025 rdf:resource="http://purl.obolibrary.org/obo/GAZ_00011616"/>
        <oboInOwl:hasOBONamespace>GAZ</oboInOwl:hasOBONamespace>
        <oboInOwl:id>GAZ:00071584</oboInOwl:id>
        <rdfs:label>Municipality of Guacara</rdfs:label>
    </owl:NamedIndividual>
    


    <!-- http://purl.obolibrary.org/obo/GAZ_00071585 -->

    <owl:NamedIndividual rdf:about="http://purl.obolibrary.org/obo/GAZ_00071585">
        <obo:RO_0001025 rdf:resource="http://purl.obolibrary.org/obo/GAZ_00011616"/>
        <oboInOwl:hasOBONamespace>GAZ</oboInOwl:hasOBONamespace>
        <oboInOwl:id>GAZ:00071585</oboInOwl:id>
        <rdfs:label>Municipality of Naguanagua</rdfs:label>
    </owl:NamedIndividual>
    


    <!-- http://purl.obolibrary.org/obo/GAZ_00071586 -->

    <owl:NamedIndividual rdf:about="http://purl.obolibrary.org/obo/GAZ_00071586">
        <obo:RO_0001025 rdf:resource="http://purl.obolibrary.org/obo/GAZ_00011616"/>
        <oboInOwl:hasOBONamespace>GAZ</oboInOwl:hasOBONamespace>
        <oboInOwl:id>GAZ:00071586</oboInOwl:id>
        <rdfs:label>Municipality of San Diego</rdfs:label>
    </owl:NamedIndividual>
    


    <!-- http://purl.obolibrary.org/obo/GAZ_00071587 -->

    <owl:NamedIndividual rdf:about="http://purl.obolibrary.org/obo/GAZ_00071587">
        <obo:RO_0001025 rdf:resource="http://purl.obolibrary.org/obo/GAZ_00011616"/>
        <oboInOwl:hasOBONamespace>GAZ</oboInOwl:hasOBONamespace>
        <oboInOwl:id>GAZ:00071587</oboInOwl:id>
        <rdfs:label>Municipality of Miranda</rdfs:label>
    </owl:NamedIndividual>
    


    <!-- http://purl.obolibrary.org/obo/GAZ_00071588 -->

    <owl:NamedIndividual rdf:about="http://purl.obolibrary.org/obo/GAZ_00071588">
        <obo:RO_0001025 rdf:resource="http://purl.obolibrary.org/obo/GAZ_00011616"/>
        <oboInOwl:hasOBONamespace>GAZ</oboInOwl:hasOBONamespace>
        <oboInOwl:id>GAZ:00071588</oboInOwl:id>
        <rdfs:label>Municipality of Juan Jose Mora</rdfs:label>
    </owl:NamedIndividual>
    


    <!-- http://purl.obolibrary.org/obo/GAZ_00071589 -->

    <owl:NamedIndividual rdf:about="http://purl.obolibrary.org/obo/GAZ_00071589">
        <obo:RO_0001025 rdf:resource="http://purl.obolibrary.org/obo/GAZ_00011616"/>
        <oboInOwl:hasOBONamespace>GAZ</oboInOwl:hasOBONamespace>
        <oboInOwl:id>GAZ:00071589</oboInOwl:id>
        <rdfs:label>Municipality of San Joaquin</rdfs:label>
    </owl:NamedIndividual>
    


    <!-- http://purl.obolibrary.org/obo/GAZ_00071590 -->

    <owl:NamedIndividual rdf:about="http://purl.obolibrary.org/obo/GAZ_00071590">
        <obo:RO_0001025 rdf:resource="http://purl.obolibrary.org/obo/GAZ_00011616"/>
        <oboInOwl:hasOBONamespace>GAZ</oboInOwl:hasOBONamespace>
        <oboInOwl:id>GAZ:00071590</oboInOwl:id>
        <rdfs:label>Municipality of Carlos Arvelo</rdfs:label>
    </owl:NamedIndividual>
    


    <!-- http://purl.obolibrary.org/obo/GAZ_00071591 -->

    <owl:NamedIndividual rdf:about="http://purl.obolibrary.org/obo/GAZ_00071591">
        <obo:RO_0001025 rdf:resource="http://purl.obolibrary.org/obo/GAZ_00011616"/>
        <oboInOwl:hasOBONamespace>GAZ</oboInOwl:hasOBONamespace>
        <oboInOwl:id>GAZ:00071591</oboInOwl:id>
        <rdfs:label>Municipality of Montalban</rdfs:label>
    </owl:NamedIndividual>
    


    <!-- http://purl.obolibrary.org/obo/GAZ_00071592 -->

    <owl:NamedIndividual rdf:about="http://purl.obolibrary.org/obo/GAZ_00071592">
        <obo:RO_0001025 rdf:resource="http://purl.obolibrary.org/obo/GAZ_00011616"/>
        <oboInOwl:hasOBONamespace>GAZ</oboInOwl:hasOBONamespace>
        <oboInOwl:id>GAZ:00071592</oboInOwl:id>
        <rdfs:label>Municipality of Puerto Cabello</rdfs:label>
    </owl:NamedIndividual>
    


    <!-- http://purl.obolibrary.org/obo/GAZ_00071593 -->

    <owl:NamedIndividual rdf:about="http://purl.obolibrary.org/obo/GAZ_00071593">
        <obo:RO_0001025 rdf:resource="http://purl.obolibrary.org/obo/GAZ_00011617"/>
        <oboInOwl:hasOBONamespace>GAZ</oboInOwl:hasOBONamespace>
        <oboInOwl:id>GAZ:00071593</oboInOwl:id>
        <rdfs:label>Municipality of Pedernales</rdfs:label>
    </owl:NamedIndividual>
    


    <!-- http://purl.obolibrary.org/obo/GAZ_00071594 -->

    <owl:NamedIndividual rdf:about="http://purl.obolibrary.org/obo/GAZ_00071594">
        <obo:RO_0001025 rdf:resource="http://purl.obolibrary.org/obo/GAZ_00011617"/>
        <oboInOwl:hasOBONamespace>GAZ</oboInOwl:hasOBONamespace>
        <oboInOwl:id>GAZ:00071594</oboInOwl:id>
        <rdfs:label>Municipality of Casacoima</rdfs:label>
    </owl:NamedIndividual>
    


    <!-- http://purl.obolibrary.org/obo/GAZ_00071595 -->

    <owl:NamedIndividual rdf:about="http://purl.obolibrary.org/obo/GAZ_00071595">
        <obo:RO_0001025 rdf:resource="http://purl.obolibrary.org/obo/GAZ_00011617"/>
        <oboInOwl:hasOBONamespace>GAZ</oboInOwl:hasOBONamespace>
        <oboInOwl:id>GAZ:00071595</oboInOwl:id>
        <rdfs:label>Municipality of Tucupita</rdfs:label>
    </owl:NamedIndividual>
    


    <!-- http://purl.obolibrary.org/obo/GAZ_00071596 -->

    <owl:NamedIndividual rdf:about="http://purl.obolibrary.org/obo/GAZ_00071596">
        <obo:RO_0001025 rdf:resource="http://purl.obolibrary.org/obo/GAZ_00011590"/>
        <oboInOwl:hasOBONamespace>GAZ</oboInOwl:hasOBONamespace>
        <oboInOwl:id>GAZ:00071596</oboInOwl:id>
        <rdfs:label>Municipality of Libertador</rdfs:label>
    </owl:NamedIndividual>
    


    <!-- http://purl.obolibrary.org/obo/GAZ_00071597 -->

    <owl:NamedIndividual rdf:about="http://purl.obolibrary.org/obo/GAZ_00071597">
        <obo:RO_0001025 rdf:resource="http://purl.obolibrary.org/obo/GAZ_00011614"/>
        <oboInOwl:hasOBONamespace>GAZ</oboInOwl:hasOBONamespace>
        <oboInOwl:id>GAZ:00071597</oboInOwl:id>
        <rdfs:label>Municipality of Urumaco</rdfs:label>
    </owl:NamedIndividual>
    


    <!-- http://purl.obolibrary.org/obo/GAZ_00071598 -->

    <owl:NamedIndividual rdf:about="http://purl.obolibrary.org/obo/GAZ_00071598">
        <obo:RO_0001025 rdf:resource="http://purl.obolibrary.org/obo/GAZ_00011614"/>
        <oboInOwl:hasOBONamespace>GAZ</oboInOwl:hasOBONamespace>
        <oboInOwl:id>GAZ:00071598</oboInOwl:id>
        <rdfs:label>Municipality of Tocopero</rdfs:label>
    </owl:NamedIndividual>
    


    <!-- http://purl.obolibrary.org/obo/GAZ_00071599 -->

    <owl:NamedIndividual rdf:about="http://purl.obolibrary.org/obo/GAZ_00071599">
        <obo:RO_0001025 rdf:resource="http://purl.obolibrary.org/obo/GAZ_00011614"/>
        <oboInOwl:hasOBONamespace>GAZ</oboInOwl:hasOBONamespace>
        <oboInOwl:id>GAZ:00071599</oboInOwl:id>
        <rdfs:label>Municipality of Zamora</rdfs:label>
    </owl:NamedIndividual>
    


    <!-- http://purl.obolibrary.org/obo/GAZ_00071600 -->

    <owl:NamedIndividual rdf:about="http://purl.obolibrary.org/obo/GAZ_00071600">
        <obo:RO_0001025 rdf:resource="http://purl.obolibrary.org/obo/GAZ_00011614"/>
        <oboInOwl:hasOBONamespace>GAZ</oboInOwl:hasOBONamespace>
        <oboInOwl:id>GAZ:00071600</oboInOwl:id>
        <rdfs:label>Municipality of Los Taques</rdfs:label>
    </owl:NamedIndividual>
    


    <!-- http://purl.obolibrary.org/obo/GAZ_00071601 -->

    <owl:NamedIndividual rdf:about="http://purl.obolibrary.org/obo/GAZ_00071601">
        <obo:RO_0001025 rdf:resource="http://purl.obolibrary.org/obo/GAZ_00011614"/>
        <oboInOwl:hasOBONamespace>GAZ</oboInOwl:hasOBONamespace>
        <oboInOwl:id>GAZ:00071601</oboInOwl:id>
        <rdfs:label>Municipality of Piritu</rdfs:label>
    </owl:NamedIndividual>
    


    <!-- http://purl.obolibrary.org/obo/GAZ_00071602 -->

    <owl:NamedIndividual rdf:about="http://purl.obolibrary.org/obo/GAZ_00071602">
        <obo:RO_0001025 rdf:resource="http://purl.obolibrary.org/obo/GAZ_00011614"/>
        <oboInOwl:hasOBONamespace>GAZ</oboInOwl:hasOBONamespace>
        <oboInOwl:id>GAZ:00071602</oboInOwl:id>
        <rdfs:label>Municipality of Colina</rdfs:label>
    </owl:NamedIndividual>
    


    <!-- http://purl.obolibrary.org/obo/GAZ_00071603 -->

    <owl:NamedIndividual rdf:about="http://purl.obolibrary.org/obo/GAZ_00071603">
        <obo:RO_0001025 rdf:resource="http://purl.obolibrary.org/obo/GAZ_00011614"/>
        <oboInOwl:hasOBONamespace>GAZ</oboInOwl:hasOBONamespace>
        <oboInOwl:id>GAZ:00071603</oboInOwl:id>
        <rdfs:label>Municipality of Buchivacoa</rdfs:label>
    </owl:NamedIndividual>
    


    <!-- http://purl.obolibrary.org/obo/GAZ_00071604 -->

    <owl:NamedIndividual rdf:about="http://purl.obolibrary.org/obo/GAZ_00071604">
        <obo:RO_0001025 rdf:resource="http://purl.obolibrary.org/obo/GAZ_00011614"/>
        <oboInOwl:hasOBONamespace>GAZ</oboInOwl:hasOBONamespace>
        <oboInOwl:id>GAZ:00071604</oboInOwl:id>
        <rdfs:label>Municipality of Cacique Manaure</rdfs:label>
    </owl:NamedIndividual>
    


    <!-- http://purl.obolibrary.org/obo/GAZ_00071605 -->

    <owl:NamedIndividual rdf:about="http://purl.obolibrary.org/obo/GAZ_00071605">
        <obo:RO_0001025 rdf:resource="http://purl.obolibrary.org/obo/GAZ_00011614"/>
        <oboInOwl:hasOBONamespace>GAZ</oboInOwl:hasOBONamespace>
        <oboInOwl:id>GAZ:00071605</oboInOwl:id>
        <rdfs:label>Municipality of Union</rdfs:label>
    </owl:NamedIndividual>
    


    <!-- http://purl.obolibrary.org/obo/GAZ_00071606 -->

    <owl:NamedIndividual rdf:about="http://purl.obolibrary.org/obo/GAZ_00071606">
        <obo:RO_0001025 rdf:resource="http://purl.obolibrary.org/obo/GAZ_00011614"/>
        <oboInOwl:hasOBONamespace>GAZ</oboInOwl:hasOBONamespace>
        <oboInOwl:id>GAZ:00071606</oboInOwl:id>
        <rdfs:label>Municipality of Falcon</rdfs:label>
    </owl:NamedIndividual>
    


    <!-- http://purl.obolibrary.org/obo/GAZ_00071607 -->

    <owl:NamedIndividual rdf:about="http://purl.obolibrary.org/obo/GAZ_00071607">
        <obo:RO_0001025 rdf:resource="http://purl.obolibrary.org/obo/GAZ_00011614"/>
        <oboInOwl:hasOBONamespace>GAZ</oboInOwl:hasOBONamespace>
        <oboInOwl:id>GAZ:00071607</oboInOwl:id>
        <rdfs:label>Municipality of Federacion</rdfs:label>
    </owl:NamedIndividual>
    


    <!-- http://purl.obolibrary.org/obo/GAZ_00071608 -->

    <owl:NamedIndividual rdf:about="http://purl.obolibrary.org/obo/GAZ_00071608">
        <obo:RO_0001025 rdf:resource="http://purl.obolibrary.org/obo/GAZ_00011614"/>
        <oboInOwl:hasOBONamespace>GAZ</oboInOwl:hasOBONamespace>
        <oboInOwl:id>GAZ:00071608</oboInOwl:id>
        <rdfs:label>Municipality of Carirubana</rdfs:label>
    </owl:NamedIndividual>
    


    <!-- http://purl.obolibrary.org/obo/GAZ_00071609 -->

    <owl:NamedIndividual rdf:about="http://purl.obolibrary.org/obo/GAZ_00071609">
        <obo:RO_0001025 rdf:resource="http://purl.obolibrary.org/obo/GAZ_00011614"/>
        <oboInOwl:hasOBONamespace>GAZ</oboInOwl:hasOBONamespace>
        <oboInOwl:id>GAZ:00071609</oboInOwl:id>
        <rdfs:label>Municipality of Bolivar</rdfs:label>
    </owl:NamedIndividual>
    


    <!-- http://purl.obolibrary.org/obo/GAZ_00071610 -->

    <owl:NamedIndividual rdf:about="http://purl.obolibrary.org/obo/GAZ_00071610">
        <obo:RO_0001025 rdf:resource="http://purl.obolibrary.org/obo/GAZ_00011614"/>
        <oboInOwl:hasOBONamespace>GAZ</oboInOwl:hasOBONamespace>
        <oboInOwl:id>GAZ:00071610</oboInOwl:id>
        <rdfs:label>Municipality of Acosta</rdfs:label>
    </owl:NamedIndividual>
    


    <!-- http://purl.obolibrary.org/obo/GAZ_00071611 -->

    <owl:NamedIndividual rdf:about="http://purl.obolibrary.org/obo/GAZ_00071611">
        <obo:RO_0001025 rdf:resource="http://purl.obolibrary.org/obo/GAZ_00011614"/>
        <oboInOwl:hasOBONamespace>GAZ</oboInOwl:hasOBONamespace>
        <oboInOwl:id>GAZ:00071611</oboInOwl:id>
        <rdfs:label>Municipality of Jacura</rdfs:label>
    </owl:NamedIndividual>
    


    <!-- http://purl.obolibrary.org/obo/GAZ_00071612 -->

    <owl:NamedIndividual rdf:about="http://purl.obolibrary.org/obo/GAZ_00071612">
        <obo:RO_0001025 rdf:resource="http://purl.obolibrary.org/obo/GAZ_00011614"/>
        <oboInOwl:hasOBONamespace>GAZ</oboInOwl:hasOBONamespace>
        <oboInOwl:id>GAZ:00071612</oboInOwl:id>
        <rdfs:label>Municipality of Dabajuro</rdfs:label>
    </owl:NamedIndividual>
    


    <!-- http://purl.obolibrary.org/obo/GAZ_00071613 -->

    <owl:NamedIndividual rdf:about="http://purl.obolibrary.org/obo/GAZ_00071613">
        <obo:RO_0001025 rdf:resource="http://purl.obolibrary.org/obo/GAZ_00011614"/>
        <oboInOwl:hasOBONamespace>GAZ</oboInOwl:hasOBONamespace>
        <oboInOwl:id>GAZ:00071613</oboInOwl:id>
        <rdfs:label>Municipality of Democracia</rdfs:label>
    </owl:NamedIndividual>
    


    <!-- http://purl.obolibrary.org/obo/GAZ_00071614 -->

    <owl:NamedIndividual rdf:about="http://purl.obolibrary.org/obo/GAZ_00071614">
        <obo:RO_0001025 rdf:resource="http://purl.obolibrary.org/obo/GAZ_00011614"/>
        <oboInOwl:hasOBONamespace>GAZ</oboInOwl:hasOBONamespace>
        <oboInOwl:id>GAZ:00071614</oboInOwl:id>
        <rdfs:label>Municipality of San Francisco</rdfs:label>
    </owl:NamedIndividual>
    


    <!-- http://purl.obolibrary.org/obo/GAZ_00071615 -->

    <owl:NamedIndividual rdf:about="http://purl.obolibrary.org/obo/GAZ_00071615">
        <obo:RO_0001025 rdf:resource="http://purl.obolibrary.org/obo/GAZ_00011614"/>
        <oboInOwl:hasOBONamespace>GAZ</oboInOwl:hasOBONamespace>
        <oboInOwl:id>GAZ:00071615</oboInOwl:id>
        <rdfs:label>Municipality of Sucre</rdfs:label>
    </owl:NamedIndividual>
    


    <!-- http://purl.obolibrary.org/obo/GAZ_00071616 -->

    <owl:NamedIndividual rdf:about="http://purl.obolibrary.org/obo/GAZ_00071616">
        <obo:RO_0001025 rdf:resource="http://purl.obolibrary.org/obo/GAZ_00011614"/>
        <oboInOwl:hasOBONamespace>GAZ</oboInOwl:hasOBONamespace>
        <oboInOwl:id>GAZ:00071616</oboInOwl:id>
        <rdfs:label>Municipality of Silva</rdfs:label>
    </owl:NamedIndividual>
    


    <!-- http://purl.obolibrary.org/obo/GAZ_00071617 -->

    <owl:NamedIndividual rdf:about="http://purl.obolibrary.org/obo/GAZ_00071617">
        <obo:RO_0001025 rdf:resource="http://purl.obolibrary.org/obo/GAZ_00011614"/>
        <oboInOwl:hasOBONamespace>GAZ</oboInOwl:hasOBONamespace>
        <oboInOwl:id>GAZ:00071617</oboInOwl:id>
        <rdfs:label>Municipality of Miranda</rdfs:label>
    </owl:NamedIndividual>
    


    <!-- http://purl.obolibrary.org/obo/GAZ_00071618 -->

    <owl:NamedIndividual rdf:about="http://purl.obolibrary.org/obo/GAZ_00071618">
        <obo:RO_0001025 rdf:resource="http://purl.obolibrary.org/obo/GAZ_00011614"/>
        <oboInOwl:hasOBONamespace>GAZ</oboInOwl:hasOBONamespace>
        <oboInOwl:id>GAZ:00071618</oboInOwl:id>
        <rdfs:label>Municipality of Palmasola</rdfs:label>
    </owl:NamedIndividual>
    


    <!-- http://purl.obolibrary.org/obo/GAZ_00071619 -->

    <owl:NamedIndividual rdf:about="http://purl.obolibrary.org/obo/GAZ_00071619">
        <obo:RO_0001025 rdf:resource="http://purl.obolibrary.org/obo/GAZ_00011614"/>
        <oboInOwl:hasOBONamespace>GAZ</oboInOwl:hasOBONamespace>
        <oboInOwl:id>GAZ:00071619</oboInOwl:id>
        <rdfs:label>Municipality of Mauroa</rdfs:label>
    </owl:NamedIndividual>
    


    <!-- http://purl.obolibrary.org/obo/GAZ_00071620 -->

    <owl:NamedIndividual rdf:about="http://purl.obolibrary.org/obo/GAZ_00071620">
        <obo:RO_0001025 rdf:resource="http://purl.obolibrary.org/obo/GAZ_00011614"/>
        <oboInOwl:hasOBONamespace>GAZ</oboInOwl:hasOBONamespace>
        <oboInOwl:id>GAZ:00071620</oboInOwl:id>
        <rdfs:label>Municipality of Petit</rdfs:label>
    </owl:NamedIndividual>
    


    <!-- http://purl.obolibrary.org/obo/GAZ_00071621 -->

    <owl:NamedIndividual rdf:about="http://purl.obolibrary.org/obo/GAZ_00071621">
        <obo:RO_0001025 rdf:resource="http://purl.obolibrary.org/obo/GAZ_00011614"/>
        <oboInOwl:hasOBONamespace>GAZ</oboInOwl:hasOBONamespace>
        <oboInOwl:id>GAZ:00071621</oboInOwl:id>
        <rdfs:label>Monsenor Iturriza</rdfs:label>
    </owl:NamedIndividual>
    


    <!-- http://purl.obolibrary.org/obo/GAZ_00071622 -->

    <owl:NamedIndividual rdf:about="http://purl.obolibrary.org/obo/GAZ_00071622">
        <obo:RO_0001025 rdf:resource="http://purl.obolibrary.org/obo/GAZ_00011595"/>
        <oboInOwl:hasOBONamespace>GAZ</oboInOwl:hasOBONamespace>
        <oboInOwl:id>GAZ:00071622</oboInOwl:id>
        <rdfs:label>Municipality of El Socorro</rdfs:label>
    </owl:NamedIndividual>
    


    <!-- http://purl.obolibrary.org/obo/GAZ_00071623 -->

    <owl:NamedIndividual rdf:about="http://purl.obolibrary.org/obo/GAZ_00071623">
        <obo:RO_0001025 rdf:resource="http://purl.obolibrary.org/obo/GAZ_00011595"/>
        <oboInOwl:hasOBONamespace>GAZ</oboInOwl:hasOBONamespace>
        <oboInOwl:id>GAZ:00071623</oboInOwl:id>
        <rdfs:label>Municipality of Jose Tadeo Monagas</rdfs:label>
    </owl:NamedIndividual>
    


    <!-- http://purl.obolibrary.org/obo/GAZ_00071624 -->

    <owl:NamedIndividual rdf:about="http://purl.obolibrary.org/obo/GAZ_00071624">
        <obo:RO_0001025 rdf:resource="http://purl.obolibrary.org/obo/GAZ_00011595"/>
        <oboInOwl:hasOBONamespace>GAZ</oboInOwl:hasOBONamespace>
        <oboInOwl:id>GAZ:00071624</oboInOwl:id>
        <rdfs:label>Municipality of Francisco de Miranda</rdfs:label>
    </owl:NamedIndividual>
    


    <!-- http://purl.obolibrary.org/obo/GAZ_00071625 -->

    <owl:NamedIndividual rdf:about="http://purl.obolibrary.org/obo/GAZ_00071625">
        <obo:RO_0001025 rdf:resource="http://purl.obolibrary.org/obo/GAZ_00011595"/>
        <oboInOwl:hasOBONamespace>GAZ</oboInOwl:hasOBONamespace>
        <oboInOwl:id>GAZ:00071625</oboInOwl:id>
        <rdfs:label>Municipality of Santa Maria de Ipire</rdfs:label>
    </owl:NamedIndividual>
    


    <!-- http://purl.obolibrary.org/obo/GAZ_00071626 -->

    <owl:NamedIndividual rdf:about="http://purl.obolibrary.org/obo/GAZ_00071626">
        <obo:RO_0001025 rdf:resource="http://purl.obolibrary.org/obo/GAZ_00011595"/>
        <oboInOwl:hasOBONamespace>GAZ</oboInOwl:hasOBONamespace>
        <oboInOwl:id>GAZ:00071626</oboInOwl:id>
        <rdfs:label>Municipality of Jose Felix Ribas</rdfs:label>
    </owl:NamedIndividual>
    


    <!-- http://purl.obolibrary.org/obo/GAZ_00071627 -->

    <owl:NamedIndividual rdf:about="http://purl.obolibrary.org/obo/GAZ_00071627">
        <obo:RO_0001025 rdf:resource="http://purl.obolibrary.org/obo/GAZ_00011595"/>
        <oboInOwl:hasOBONamespace>GAZ</oboInOwl:hasOBONamespace>
        <oboInOwl:id>GAZ:00071627</oboInOwl:id>
        <rdfs:label>Municipality of Pedro Zaraza</rdfs:label>
    </owl:NamedIndividual>
    


    <!-- http://purl.obolibrary.org/obo/GAZ_00071628 -->

    <owl:NamedIndividual rdf:about="http://purl.obolibrary.org/obo/GAZ_00071628">
        <obo:RO_0001025 rdf:resource="http://purl.obolibrary.org/obo/GAZ_00011595"/>
        <oboInOwl:hasOBONamespace>GAZ</oboInOwl:hasOBONamespace>
        <oboInOwl:id>GAZ:00071628</oboInOwl:id>
        <rdfs:label>Municipality of Camaguan</rdfs:label>
    </owl:NamedIndividual>
    


    <!-- http://purl.obolibrary.org/obo/GAZ_00071629 -->

    <owl:NamedIndividual rdf:about="http://purl.obolibrary.org/obo/GAZ_00071629">
        <obo:RO_0001025 rdf:resource="http://purl.obolibrary.org/obo/GAZ_00011595"/>
        <oboInOwl:hasOBONamespace>GAZ</oboInOwl:hasOBONamespace>
        <oboInOwl:id>GAZ:00071629</oboInOwl:id>
        <rdfs:label>Municipality of Julian Mellado</rdfs:label>
    </owl:NamedIndividual>
    


    <!-- http://purl.obolibrary.org/obo/GAZ_00071630 -->

    <owl:NamedIndividual rdf:about="http://purl.obolibrary.org/obo/GAZ_00071630">
        <obo:RO_0001025 rdf:resource="http://purl.obolibrary.org/obo/GAZ_00011595"/>
        <oboInOwl:hasOBONamespace>GAZ</oboInOwl:hasOBONamespace>
        <oboInOwl:id>GAZ:00071630</oboInOwl:id>
        <rdfs:label>Municipality of Leonardo Infante</rdfs:label>
    </owl:NamedIndividual>
    


    <!-- http://purl.obolibrary.org/obo/GAZ_00071631 -->

    <owl:NamedIndividual rdf:about="http://purl.obolibrary.org/obo/GAZ_00071631">
        <obo:RO_0001025 rdf:resource="http://purl.obolibrary.org/obo/GAZ_00011595"/>
        <oboInOwl:hasOBONamespace>GAZ</oboInOwl:hasOBONamespace>
        <oboInOwl:id>GAZ:00071631</oboInOwl:id>
        <rdfs:label>Municipality of San Geronimo de Guayabal</rdfs:label>
    </owl:NamedIndividual>
    


    <!-- http://purl.obolibrary.org/obo/GAZ_00071632 -->

    <owl:NamedIndividual rdf:about="http://purl.obolibrary.org/obo/GAZ_00071632">
        <obo:RO_0001025 rdf:resource="http://purl.obolibrary.org/obo/GAZ_00011595"/>
        <oboInOwl:hasOBONamespace>GAZ</oboInOwl:hasOBONamespace>
        <oboInOwl:id>GAZ:00071632</oboInOwl:id>
        <rdfs:label>Municipality of Chaguaramas</rdfs:label>
    </owl:NamedIndividual>
    


    <!-- http://purl.obolibrary.org/obo/GAZ_00071633 -->

    <owl:NamedIndividual rdf:about="http://purl.obolibrary.org/obo/GAZ_00071633">
        <obo:RO_0001025 rdf:resource="http://purl.obolibrary.org/obo/GAZ_00011595"/>
        <oboInOwl:hasOBONamespace>GAZ</oboInOwl:hasOBONamespace>
        <oboInOwl:id>GAZ:00071633</oboInOwl:id>
        <rdfs:label>Municipality of Ortiz</rdfs:label>
    </owl:NamedIndividual>
    


    <!-- http://purl.obolibrary.org/obo/GAZ_00071634 -->

    <owl:NamedIndividual rdf:about="http://purl.obolibrary.org/obo/GAZ_00071634">
        <obo:RO_0001025 rdf:resource="http://purl.obolibrary.org/obo/GAZ_00011595"/>
        <oboInOwl:hasOBONamespace>GAZ</oboInOwl:hasOBONamespace>
        <oboInOwl:id>GAZ:00071634</oboInOwl:id>
        <rdfs:label>Municipality of San Jose de Guaribe</rdfs:label>
    </owl:NamedIndividual>
    


    <!-- http://purl.obolibrary.org/obo/GAZ_00071635 -->

    <owl:NamedIndividual rdf:about="http://purl.obolibrary.org/obo/GAZ_00071635">
        <obo:RO_0001025 rdf:resource="http://purl.obolibrary.org/obo/GAZ_00011595"/>
        <oboInOwl:hasOBONamespace>GAZ</oboInOwl:hasOBONamespace>
        <oboInOwl:id>GAZ:00071635</oboInOwl:id>
        <rdfs:label>Municipality of Las Mercedes</rdfs:label>
    </owl:NamedIndividual>
    


    <!-- http://purl.obolibrary.org/obo/GAZ_00071636 -->

    <owl:NamedIndividual rdf:about="http://purl.obolibrary.org/obo/GAZ_00071636">
        <obo:RO_0001025 rdf:resource="http://purl.obolibrary.org/obo/GAZ_00011595"/>
        <oboInOwl:hasOBONamespace>GAZ</oboInOwl:hasOBONamespace>
        <oboInOwl:id>GAZ:00071636</oboInOwl:id>
        <rdfs:label>Municipality of Juan German Roscio</rdfs:label>
    </owl:NamedIndividual>
    


    <!-- http://purl.obolibrary.org/obo/GAZ_00071637 -->

    <owl:NamedIndividual rdf:about="http://purl.obolibrary.org/obo/GAZ_00071637">
        <obo:RO_0001025 rdf:resource="http://purl.obolibrary.org/obo/GAZ_00011623"/>
        <oboInOwl:hasOBONamespace>GAZ</oboInOwl:hasOBONamespace>
        <oboInOwl:id>GAZ:00071637</oboInOwl:id>
        <rdfs:label>Municipality of Simon Planas</rdfs:label>
    </owl:NamedIndividual>
    


    <!-- http://purl.obolibrary.org/obo/GAZ_00071638 -->

    <owl:NamedIndividual rdf:about="http://purl.obolibrary.org/obo/GAZ_00071638">
        <obo:RO_0001025 rdf:resource="http://purl.obolibrary.org/obo/GAZ_00011623"/>
        <oboInOwl:hasOBONamespace>GAZ</oboInOwl:hasOBONamespace>
        <oboInOwl:id>GAZ:00071638</oboInOwl:id>
        <rdfs:label>Municipality of Crespo</rdfs:label>
    </owl:NamedIndividual>
    


    <!-- http://purl.obolibrary.org/obo/GAZ_00071639 -->

    <owl:NamedIndividual rdf:about="http://purl.obolibrary.org/obo/GAZ_00071639">
        <obo:RO_0001025 rdf:resource="http://purl.obolibrary.org/obo/GAZ_00011623"/>
        <oboInOwl:hasOBONamespace>GAZ</oboInOwl:hasOBONamespace>
        <oboInOwl:id>GAZ:00071639</oboInOwl:id>
        <rdfs:label>Municipality of Urdaneta</rdfs:label>
    </owl:NamedIndividual>
    


    <!-- http://purl.obolibrary.org/obo/GAZ_00071640 -->

    <owl:NamedIndividual rdf:about="http://purl.obolibrary.org/obo/GAZ_00071640">
        <obo:RO_0001025 rdf:resource="http://purl.obolibrary.org/obo/GAZ_00011623"/>
        <oboInOwl:hasOBONamespace>GAZ</oboInOwl:hasOBONamespace>
        <oboInOwl:id>GAZ:00071640</oboInOwl:id>
        <rdfs:label>Municipality of Jimenez</rdfs:label>
    </owl:NamedIndividual>
    


    <!-- http://purl.obolibrary.org/obo/GAZ_00071641 -->

    <owl:NamedIndividual rdf:about="http://purl.obolibrary.org/obo/GAZ_00071641">
        <obo:RO_0001025 rdf:resource="http://purl.obolibrary.org/obo/GAZ_00011623"/>
        <oboInOwl:hasOBONamespace>GAZ</oboInOwl:hasOBONamespace>
        <oboInOwl:id>GAZ:00071641</oboInOwl:id>
        <rdfs:label>Municipality of Andres Eloy</rdfs:label>
    </owl:NamedIndividual>
    


    <!-- http://purl.obolibrary.org/obo/GAZ_00071642 -->

    <owl:NamedIndividual rdf:about="http://purl.obolibrary.org/obo/GAZ_00071642">
        <obo:RO_0001025 rdf:resource="http://purl.obolibrary.org/obo/GAZ_00011623"/>
        <oboInOwl:hasOBONamespace>GAZ</oboInOwl:hasOBONamespace>
        <oboInOwl:id>GAZ:00071642</oboInOwl:id>
        <rdfs:label>Municipality of Blanco</rdfs:label>
    </owl:NamedIndividual>
    


    <!-- http://purl.obolibrary.org/obo/GAZ_00071643 -->

    <owl:NamedIndividual rdf:about="http://purl.obolibrary.org/obo/GAZ_00071643">
        <obo:RO_0001025 rdf:resource="http://purl.obolibrary.org/obo/GAZ_00011623"/>
        <oboInOwl:hasOBONamespace>GAZ</oboInOwl:hasOBONamespace>
        <oboInOwl:id>GAZ:00071643</oboInOwl:id>
        <rdfs:label>Municipality of Moran</rdfs:label>
    </owl:NamedIndividual>
    


    <!-- http://purl.obolibrary.org/obo/GAZ_00071644 -->

    <owl:NamedIndividual rdf:about="http://purl.obolibrary.org/obo/GAZ_00071644">
        <obo:RO_0001025 rdf:resource="http://purl.obolibrary.org/obo/GAZ_00011623"/>
        <oboInOwl:hasOBONamespace>GAZ</oboInOwl:hasOBONamespace>
        <oboInOwl:id>GAZ:00071644</oboInOwl:id>
        <rdfs:label>Municipality of Iribarren</rdfs:label>
    </owl:NamedIndividual>
    


    <!-- http://purl.obolibrary.org/obo/GAZ_00071645 -->

    <owl:NamedIndividual rdf:about="http://purl.obolibrary.org/obo/GAZ_00071645">
        <obo:RO_0001025 rdf:resource="http://purl.obolibrary.org/obo/GAZ_00011623"/>
        <oboInOwl:hasOBONamespace>GAZ</oboInOwl:hasOBONamespace>
        <oboInOwl:id>GAZ:00071645</oboInOwl:id>
        <rdfs:label>Municipality of Palavecino</rdfs:label>
    </owl:NamedIndividual>
    


    <!-- http://purl.obolibrary.org/obo/GAZ_00071646 -->

    <owl:NamedIndividual rdf:about="http://purl.obolibrary.org/obo/GAZ_00071646">
        <obo:RO_0001025 rdf:resource="http://purl.obolibrary.org/obo/GAZ_00011623"/>
        <oboInOwl:hasOBONamespace>GAZ</oboInOwl:hasOBONamespace>
        <oboInOwl:id>GAZ:00071646</oboInOwl:id>
        <rdfs:label>Municipality of Torres</rdfs:label>
    </owl:NamedIndividual>
    


    <!-- http://purl.obolibrary.org/obo/GAZ_00071647 -->

    <owl:NamedIndividual rdf:about="http://purl.obolibrary.org/obo/GAZ_00071647">
        <obo:RO_0001025 rdf:resource="http://purl.obolibrary.org/obo/GAZ_00011621"/>
        <oboInOwl:hasOBONamespace>GAZ</oboInOwl:hasOBONamespace>
        <oboInOwl:id>GAZ:00071647</oboInOwl:id>
        <rdfs:label>Municipality of Sucre</rdfs:label>
    </owl:NamedIndividual>
    


    <!-- http://purl.obolibrary.org/obo/GAZ_00071648 -->

    <owl:NamedIndividual rdf:about="http://purl.obolibrary.org/obo/GAZ_00071648">
        <obo:RO_0001025 rdf:resource="http://purl.obolibrary.org/obo/GAZ_00011621"/>
        <oboInOwl:hasOBONamespace>GAZ</oboInOwl:hasOBONamespace>
        <oboInOwl:id>GAZ:00071648</oboInOwl:id>
        <rdfs:label>Municipality of Cardenal Quintero</rdfs:label>
    </owl:NamedIndividual>
    


    <!-- http://purl.obolibrary.org/obo/GAZ_00071649 -->

    <owl:NamedIndividual rdf:about="http://purl.obolibrary.org/obo/GAZ_00071649">
        <obo:RO_0001025 rdf:resource="http://purl.obolibrary.org/obo/GAZ_00011621"/>
        <oboInOwl:hasOBONamespace>GAZ</oboInOwl:hasOBONamespace>
        <oboInOwl:id>GAZ:00071649</oboInOwl:id>
        <rdfs:label>Municipality of Antonio Pinto Salinas</rdfs:label>
    </owl:NamedIndividual>
    


    <!-- http://purl.obolibrary.org/obo/GAZ_00071650 -->

    <owl:NamedIndividual rdf:about="http://purl.obolibrary.org/obo/GAZ_00071650">
        <obo:RO_0001025 rdf:resource="http://purl.obolibrary.org/obo/GAZ_00011621"/>
        <oboInOwl:hasOBONamespace>GAZ</oboInOwl:hasOBONamespace>
        <oboInOwl:id>GAZ:00071650</oboInOwl:id>
        <rdfs:label>Municipality of Aricagua</rdfs:label>
    </owl:NamedIndividual>
    


    <!-- http://purl.obolibrary.org/obo/GAZ_00071651 -->

    <owl:NamedIndividual rdf:about="http://purl.obolibrary.org/obo/GAZ_00071651">
        <obo:RO_0001025 rdf:resource="http://purl.obolibrary.org/obo/GAZ_00011621"/>
        <oboInOwl:hasOBONamespace>GAZ</oboInOwl:hasOBONamespace>
        <oboInOwl:id>GAZ:00071651</oboInOwl:id>
        <rdfs:label>Municipality of Libertador</rdfs:label>
    </owl:NamedIndividual>
    


    <!-- http://purl.obolibrary.org/obo/GAZ_00071652 -->

    <owl:NamedIndividual rdf:about="http://purl.obolibrary.org/obo/GAZ_00071652">
        <obo:RO_0001025 rdf:resource="http://purl.obolibrary.org/obo/GAZ_00011621"/>
        <oboInOwl:hasOBONamespace>GAZ</oboInOwl:hasOBONamespace>
        <oboInOwl:id>GAZ:00071652</oboInOwl:id>
        <rdfs:label>Municipality of Campo Elias</rdfs:label>
    </owl:NamedIndividual>
    


    <!-- http://purl.obolibrary.org/obo/GAZ_00071653 -->

    <owl:NamedIndividual rdf:about="http://purl.obolibrary.org/obo/GAZ_00071653">
        <obo:RO_0001025 rdf:resource="http://purl.obolibrary.org/obo/GAZ_00011621"/>
        <oboInOwl:hasOBONamespace>GAZ</oboInOwl:hasOBONamespace>
        <oboInOwl:id>GAZ:00071653</oboInOwl:id>
        <rdfs:label>Municipality of Obispo Ramos de Lora</rdfs:label>
    </owl:NamedIndividual>
    


    <!-- http://purl.obolibrary.org/obo/GAZ_00071654 -->

    <owl:NamedIndividual rdf:about="http://purl.obolibrary.org/obo/GAZ_00071654">
        <obo:RO_0001025 rdf:resource="http://purl.obolibrary.org/obo/GAZ_00011621"/>
        <oboInOwl:hasOBONamespace>GAZ</oboInOwl:hasOBONamespace>
        <oboInOwl:id>GAZ:00071654</oboInOwl:id>
        <rdfs:label>Municipality of Padre Noguera</rdfs:label>
    </owl:NamedIndividual>
    


    <!-- http://purl.obolibrary.org/obo/GAZ_00071655 -->

    <owl:NamedIndividual rdf:about="http://purl.obolibrary.org/obo/GAZ_00071655">
        <obo:RO_0001025 rdf:resource="http://purl.obolibrary.org/obo/GAZ_00011621"/>
        <oboInOwl:hasOBONamespace>GAZ</oboInOwl:hasOBONamespace>
        <oboInOwl:id>GAZ:00071655</oboInOwl:id>
        <rdfs:label>Municipality of Alberto Adriani</rdfs:label>
    </owl:NamedIndividual>
    


    <!-- http://purl.obolibrary.org/obo/GAZ_00071656 -->

    <owl:NamedIndividual rdf:about="http://purl.obolibrary.org/obo/GAZ_00071656">
        <obo:RO_0001025 rdf:resource="http://purl.obolibrary.org/obo/GAZ_00011621"/>
        <oboInOwl:hasOBONamespace>GAZ</oboInOwl:hasOBONamespace>
        <oboInOwl:id>GAZ:00071656</oboInOwl:id>
        <rdfs:label>Municipality of Justo Briceno</rdfs:label>
    </owl:NamedIndividual>
    


    <!-- http://purl.obolibrary.org/obo/GAZ_00071657 -->

    <owl:NamedIndividual rdf:about="http://purl.obolibrary.org/obo/GAZ_00071657">
        <obo:RO_0001025 rdf:resource="http://purl.obolibrary.org/obo/GAZ_00011621"/>
        <oboInOwl:hasOBONamespace>GAZ</oboInOwl:hasOBONamespace>
        <oboInOwl:id>GAZ:00071657</oboInOwl:id>
        <rdfs:label>Municipality of Andres Bello</rdfs:label>
    </owl:NamedIndividual>
    


    <!-- http://purl.obolibrary.org/obo/GAZ_00071658 -->

    <owl:NamedIndividual rdf:about="http://purl.obolibrary.org/obo/GAZ_00071658">
        <obo:RO_0001025 rdf:resource="http://purl.obolibrary.org/obo/GAZ_00011621"/>
        <oboInOwl:hasOBONamespace>GAZ</oboInOwl:hasOBONamespace>
        <oboInOwl:id>GAZ:00071658</oboInOwl:id>
        <rdfs:label>Municipality of Arzobispo Chacon</rdfs:label>
    </owl:NamedIndividual>
    


    <!-- http://purl.obolibrary.org/obo/GAZ_00071659 -->

    <owl:NamedIndividual rdf:about="http://purl.obolibrary.org/obo/GAZ_00071659">
        <obo:RO_0001025 rdf:resource="http://purl.obolibrary.org/obo/GAZ_00011621"/>
        <oboInOwl:hasOBONamespace>GAZ</oboInOwl:hasOBONamespace>
        <oboInOwl:id>GAZ:00071659</oboInOwl:id>
        <rdfs:label>Municipality of Zea</rdfs:label>
    </owl:NamedIndividual>
    


    <!-- http://purl.obolibrary.org/obo/GAZ_00071660 -->

    <owl:NamedIndividual rdf:about="http://purl.obolibrary.org/obo/GAZ_00071660">
        <obo:RO_0001025 rdf:resource="http://purl.obolibrary.org/obo/GAZ_00011621"/>
        <oboInOwl:hasOBONamespace>GAZ</oboInOwl:hasOBONamespace>
        <oboInOwl:id>GAZ:00071660</oboInOwl:id>
        <rdfs:label>Municipality of Santos Marquina</rdfs:label>
    </owl:NamedIndividual>
    


    <!-- http://purl.obolibrary.org/obo/GAZ_00071661 -->

    <owl:NamedIndividual rdf:about="http://purl.obolibrary.org/obo/GAZ_00071661">
        <obo:RO_0001025 rdf:resource="http://purl.obolibrary.org/obo/GAZ_00011621"/>
        <oboInOwl:hasOBONamespace>GAZ</oboInOwl:hasOBONamespace>
        <oboInOwl:id>GAZ:00071661</oboInOwl:id>
        <rdfs:label>Municipality of Pueblo Llano</rdfs:label>
    </owl:NamedIndividual>
    


    <!-- http://purl.obolibrary.org/obo/GAZ_00071662 -->

    <owl:NamedIndividual rdf:about="http://purl.obolibrary.org/obo/GAZ_00071662">
        <obo:RO_0001025 rdf:resource="http://purl.obolibrary.org/obo/GAZ_00011621"/>
        <oboInOwl:hasOBONamespace>GAZ</oboInOwl:hasOBONamespace>
        <oboInOwl:id>GAZ:00071662</oboInOwl:id>
        <rdfs:label>Municipality of Julio Cesar Salas</rdfs:label>
    </owl:NamedIndividual>
    


    <!-- http://purl.obolibrary.org/obo/GAZ_00071663 -->

    <owl:NamedIndividual rdf:about="http://purl.obolibrary.org/obo/GAZ_00071663">
        <obo:RO_0001025 rdf:resource="http://purl.obolibrary.org/obo/GAZ_00011621"/>
        <oboInOwl:hasOBONamespace>GAZ</oboInOwl:hasOBONamespace>
        <oboInOwl:id>GAZ:00071663</oboInOwl:id>
        <rdfs:label>Municipality of Rangel</rdfs:label>
    </owl:NamedIndividual>
    


    <!-- http://purl.obolibrary.org/obo/GAZ_00071664 -->

    <owl:NamedIndividual rdf:about="http://purl.obolibrary.org/obo/GAZ_00071664">
        <obo:RO_0001025 rdf:resource="http://purl.obolibrary.org/obo/GAZ_00011621"/>
        <oboInOwl:hasOBONamespace>GAZ</oboInOwl:hasOBONamespace>
        <oboInOwl:id>GAZ:00071664</oboInOwl:id>
        <rdfs:label>Municipality of Rivas Davila</rdfs:label>
    </owl:NamedIndividual>
    


    <!-- http://purl.obolibrary.org/obo/GAZ_00071665 -->

    <owl:NamedIndividual rdf:about="http://purl.obolibrary.org/obo/GAZ_00071665">
        <obo:RO_0001025 rdf:resource="http://purl.obolibrary.org/obo/GAZ_00011621"/>
        <oboInOwl:hasOBONamespace>GAZ</oboInOwl:hasOBONamespace>
        <oboInOwl:id>GAZ:00071665</oboInOwl:id>
        <rdfs:label>Municipality of Guaraque</rdfs:label>
    </owl:NamedIndividual>
    


    <!-- http://purl.obolibrary.org/obo/GAZ_00071666 -->

    <owl:NamedIndividual rdf:about="http://purl.obolibrary.org/obo/GAZ_00071666">
        <obo:RO_0001025 rdf:resource="http://purl.obolibrary.org/obo/GAZ_00011621"/>
        <oboInOwl:hasOBONamespace>GAZ</oboInOwl:hasOBONamespace>
        <oboInOwl:id>GAZ:00071666</oboInOwl:id>
        <rdfs:label>Municipality of Tovar</rdfs:label>
    </owl:NamedIndividual>
    


    <!-- http://purl.obolibrary.org/obo/GAZ_00071667 -->

    <owl:NamedIndividual rdf:about="http://purl.obolibrary.org/obo/GAZ_00071667">
        <obo:RO_0001025 rdf:resource="http://purl.obolibrary.org/obo/GAZ_00011621"/>
        <oboInOwl:hasOBONamespace>GAZ</oboInOwl:hasOBONamespace>
        <oboInOwl:id>GAZ:00071667</oboInOwl:id>
        <rdfs:label>Municipality of Tulio Febres Cordero</rdfs:label>
    </owl:NamedIndividual>
    


    <!-- http://purl.obolibrary.org/obo/GAZ_00071668 -->

    <owl:NamedIndividual rdf:about="http://purl.obolibrary.org/obo/GAZ_00071668">
        <obo:RO_0001025 rdf:resource="http://purl.obolibrary.org/obo/GAZ_00011621"/>
        <oboInOwl:hasOBONamespace>GAZ</oboInOwl:hasOBONamespace>
        <oboInOwl:id>GAZ:00071668</oboInOwl:id>
        <rdfs:label>Municipality of Caracciolo Parra Olmedo</rdfs:label>
    </owl:NamedIndividual>
    


    <!-- http://purl.obolibrary.org/obo/GAZ_00071669 -->

    <owl:NamedIndividual rdf:about="http://purl.obolibrary.org/obo/GAZ_00071669">
        <obo:RO_0001025 rdf:resource="http://purl.obolibrary.org/obo/GAZ_00011621"/>
        <oboInOwl:hasOBONamespace>GAZ</oboInOwl:hasOBONamespace>
        <oboInOwl:id>GAZ:00071669</oboInOwl:id>
        <rdfs:label>Municipality of Miranda</rdfs:label>
    </owl:NamedIndividual>
    


    <!-- http://purl.obolibrary.org/obo/GAZ_00072025 -->

    <owl:NamedIndividual rdf:about="http://purl.obolibrary.org/obo/GAZ_00072025">
        <obo:RO_0001025 rdf:resource="http://purl.obolibrary.org/obo/GAZ_00011622"/>
        <oboInOwl:hasOBONamespace>GAZ</oboInOwl:hasOBONamespace>
        <oboInOwl:id>GAZ:00072025</oboInOwl:id>
        <rdfs:label>Municipality of Acevedo</rdfs:label>
    </owl:NamedIndividual>
    


    <!-- http://purl.obolibrary.org/obo/GAZ_00072026 -->

    <owl:NamedIndividual rdf:about="http://purl.obolibrary.org/obo/GAZ_00072026">
        <obo:RO_0001025 rdf:resource="http://purl.obolibrary.org/obo/GAZ_00011622"/>
        <oboInOwl:hasOBONamespace>GAZ</oboInOwl:hasOBONamespace>
        <oboInOwl:id>GAZ:00072026</oboInOwl:id>
        <rdfs:label>Municipality of Plaza</rdfs:label>
    </owl:NamedIndividual>
    


    <!-- http://purl.obolibrary.org/obo/GAZ_00072027 -->

    <owl:NamedIndividual rdf:about="http://purl.obolibrary.org/obo/GAZ_00072027">
        <obo:RO_0001025 rdf:resource="http://purl.obolibrary.org/obo/GAZ_00011622"/>
        <oboInOwl:hasOBONamespace>GAZ</oboInOwl:hasOBONamespace>
        <oboInOwl:id>GAZ:00072027</oboInOwl:id>
        <rdfs:label>Municipality of Zamora</rdfs:label>
    </owl:NamedIndividual>
    


    <!-- http://purl.obolibrary.org/obo/GAZ_00072028 -->

    <owl:NamedIndividual rdf:about="http://purl.obolibrary.org/obo/GAZ_00072028">
        <obo:RO_0001025 rdf:resource="http://purl.obolibrary.org/obo/GAZ_00011622"/>
        <oboInOwl:hasOBONamespace>GAZ</oboInOwl:hasOBONamespace>
        <oboInOwl:id>GAZ:00072028</oboInOwl:id>
        <rdfs:label>Municipality of Paz Castillo</rdfs:label>
    </owl:NamedIndividual>
    


    <!-- http://purl.obolibrary.org/obo/GAZ_00072029 -->

    <owl:NamedIndividual rdf:about="http://purl.obolibrary.org/obo/GAZ_00072029">
        <obo:RO_0001025 rdf:resource="http://purl.obolibrary.org/obo/GAZ_00011622"/>
        <oboInOwl:hasOBONamespace>GAZ</oboInOwl:hasOBONamespace>
        <oboInOwl:id>GAZ:00072029</oboInOwl:id>
        <rdfs:label>Municipality of Simon Bolivar</rdfs:label>
    </owl:NamedIndividual>
    


    <!-- http://purl.obolibrary.org/obo/GAZ_00072030 -->

    <owl:NamedIndividual rdf:about="http://purl.obolibrary.org/obo/GAZ_00072030">
        <obo:RO_0001025 rdf:resource="http://purl.obolibrary.org/obo/GAZ_00011622"/>
        <oboInOwl:hasOBONamespace>GAZ</oboInOwl:hasOBONamespace>
        <oboInOwl:id>GAZ:00072030</oboInOwl:id>
        <rdfs:label>Municipality of Andres Bello</rdfs:label>
    </owl:NamedIndividual>
    


    <!-- http://purl.obolibrary.org/obo/GAZ_00072031 -->

    <owl:NamedIndividual rdf:about="http://purl.obolibrary.org/obo/GAZ_00072031">
        <obo:RO_0001025 rdf:resource="http://purl.obolibrary.org/obo/GAZ_00011622"/>
        <oboInOwl:hasOBONamespace>GAZ</oboInOwl:hasOBONamespace>
        <oboInOwl:id>GAZ:00072031</oboInOwl:id>
        <rdfs:label>Municipality of Urdaneta</rdfs:label>
    </owl:NamedIndividual>
    


    <!-- http://purl.obolibrary.org/obo/GAZ_00072032 -->

    <owl:NamedIndividual rdf:about="http://purl.obolibrary.org/obo/GAZ_00072032">
        <obo:RO_0001025 rdf:resource="http://purl.obolibrary.org/obo/GAZ_00011622"/>
        <oboInOwl:hasOBONamespace>GAZ</oboInOwl:hasOBONamespace>
        <oboInOwl:id>GAZ:00072032</oboInOwl:id>
        <rdfs:label>Municipality of Brion</rdfs:label>
    </owl:NamedIndividual>
    


    <!-- http://purl.obolibrary.org/obo/GAZ_00072033 -->

    <owl:NamedIndividual rdf:about="http://purl.obolibrary.org/obo/GAZ_00072033">
        <obo:RO_0001025 rdf:resource="http://purl.obolibrary.org/obo/GAZ_00011622"/>
        <oboInOwl:hasOBONamespace>GAZ</oboInOwl:hasOBONamespace>
        <oboInOwl:id>GAZ:00072033</oboInOwl:id>
        <rdfs:label>Municipality of Paez</rdfs:label>
    </owl:NamedIndividual>
    


    <!-- http://purl.obolibrary.org/obo/GAZ_00072034 -->

    <owl:NamedIndividual rdf:about="http://purl.obolibrary.org/obo/GAZ_00072034">
        <obo:RO_0001025 rdf:resource="http://purl.obolibrary.org/obo/GAZ_00011622"/>
        <oboInOwl:hasOBONamespace>GAZ</oboInOwl:hasOBONamespace>
        <oboInOwl:id>GAZ:00072034</oboInOwl:id>
        <rdfs:label>Municipality of Baruta</rdfs:label>
    </owl:NamedIndividual>
    


    <!-- http://purl.obolibrary.org/obo/GAZ_00072035 -->

    <owl:NamedIndividual rdf:about="http://purl.obolibrary.org/obo/GAZ_00072035">
        <obo:RO_0001025 rdf:resource="http://purl.obolibrary.org/obo/GAZ_00011622"/>
        <oboInOwl:hasOBONamespace>GAZ</oboInOwl:hasOBONamespace>
        <oboInOwl:id>GAZ:00072035</oboInOwl:id>
        <rdfs:label>Municipality of Cristobal Rojas</rdfs:label>
    </owl:NamedIndividual>
    


    <!-- http://purl.obolibrary.org/obo/GAZ_00072036 -->

    <owl:NamedIndividual rdf:about="http://purl.obolibrary.org/obo/GAZ_00072036">
        <obo:RO_0001025 rdf:resource="http://purl.obolibrary.org/obo/GAZ_00011622"/>
        <oboInOwl:hasOBONamespace>GAZ</oboInOwl:hasOBONamespace>
        <oboInOwl:id>GAZ:00072036</oboInOwl:id>
        <rdfs:label>Municipality of Chacao</rdfs:label>
    </owl:NamedIndividual>
    


    <!-- http://purl.obolibrary.org/obo/GAZ_00072037 -->

    <owl:NamedIndividual rdf:about="http://purl.obolibrary.org/obo/GAZ_00072037">
        <obo:RO_0001025 rdf:resource="http://purl.obolibrary.org/obo/GAZ_00011622"/>
        <oboInOwl:hasOBONamespace>GAZ</oboInOwl:hasOBONamespace>
        <oboInOwl:id>GAZ:00072037</oboInOwl:id>
        <rdfs:label>Municipality of Sucre</rdfs:label>
    </owl:NamedIndividual>
    


    <!-- http://purl.obolibrary.org/obo/GAZ_00072038 -->

    <owl:NamedIndividual rdf:about="http://purl.obolibrary.org/obo/GAZ_00072038">
        <obo:RO_0001025 rdf:resource="http://purl.obolibrary.org/obo/GAZ_00011622"/>
        <oboInOwl:hasOBONamespace>GAZ</oboInOwl:hasOBONamespace>
        <oboInOwl:id>GAZ:00072038</oboInOwl:id>
        <rdfs:label>Municipality of Carrizal</rdfs:label>
    </owl:NamedIndividual>
    


    <!-- http://purl.obolibrary.org/obo/GAZ_00072039 -->

    <owl:NamedIndividual rdf:about="http://purl.obolibrary.org/obo/GAZ_00072039">
        <obo:RO_0001025 rdf:resource="http://purl.obolibrary.org/obo/GAZ_00011622"/>
        <oboInOwl:hasOBONamespace>GAZ</oboInOwl:hasOBONamespace>
        <oboInOwl:id>GAZ:00072039</oboInOwl:id>
        <rdfs:label>Municipality of Guaicaipuro</rdfs:label>
    </owl:NamedIndividual>
    


    <!-- http://purl.obolibrary.org/obo/GAZ_00072040 -->

    <owl:NamedIndividual rdf:about="http://purl.obolibrary.org/obo/GAZ_00072040">
        <obo:RO_0001025 rdf:resource="http://purl.obolibrary.org/obo/GAZ_00011622"/>
        <oboInOwl:hasOBONamespace>GAZ</oboInOwl:hasOBONamespace>
        <oboInOwl:id>GAZ:00072040</oboInOwl:id>
        <rdfs:label>Municipality of El Hatillo</rdfs:label>
    </owl:NamedIndividual>
    


    <!-- http://purl.obolibrary.org/obo/GAZ_00072041 -->

    <owl:NamedIndividual rdf:about="http://purl.obolibrary.org/obo/GAZ_00072041">
        <obo:RO_0001025 rdf:resource="http://purl.obolibrary.org/obo/GAZ_00011622"/>
        <oboInOwl:hasOBONamespace>GAZ</oboInOwl:hasOBONamespace>
        <oboInOwl:id>GAZ:00072041</oboInOwl:id>
        <rdfs:label>Municipality of Lander</rdfs:label>
    </owl:NamedIndividual>
    


    <!-- http://purl.obolibrary.org/obo/GAZ_00072042 -->

    <owl:NamedIndividual rdf:about="http://purl.obolibrary.org/obo/GAZ_00072042">
        <obo:RO_0001025 rdf:resource="http://purl.obolibrary.org/obo/GAZ_00011622"/>
        <oboInOwl:hasOBONamespace>GAZ</oboInOwl:hasOBONamespace>
        <oboInOwl:id>GAZ:00072042</oboInOwl:id>
        <rdfs:label>Municipality of Buroz</rdfs:label>
    </owl:NamedIndividual>
    


    <!-- http://purl.obolibrary.org/obo/GAZ_00072043 -->

    <owl:NamedIndividual rdf:about="http://purl.obolibrary.org/obo/GAZ_00072043">
        <obo:RO_0001025 rdf:resource="http://purl.obolibrary.org/obo/GAZ_00011622"/>
        <oboInOwl:hasOBONamespace>GAZ</oboInOwl:hasOBONamespace>
        <oboInOwl:id>GAZ:00072043</oboInOwl:id>
        <rdfs:label>Municipality of Pedro Gual</rdfs:label>
    </owl:NamedIndividual>
    


    <!-- http://purl.obolibrary.org/obo/GAZ_00072044 -->

    <owl:NamedIndividual rdf:about="http://purl.obolibrary.org/obo/GAZ_00072044">
        <obo:RO_0001025 rdf:resource="http://purl.obolibrary.org/obo/GAZ_00011622"/>
        <oboInOwl:hasOBONamespace>GAZ</oboInOwl:hasOBONamespace>
        <oboInOwl:id>GAZ:00072044</oboInOwl:id>
        <rdfs:label>Municipality of Independencia</rdfs:label>
    </owl:NamedIndividual>
    


    <!-- http://purl.obolibrary.org/obo/GAZ_00072045 -->

    <owl:NamedIndividual rdf:about="http://purl.obolibrary.org/obo/GAZ_00072045">
        <obo:RO_0001025 rdf:resource="http://purl.obolibrary.org/obo/GAZ_00011622"/>
        <oboInOwl:hasOBONamespace>GAZ</oboInOwl:hasOBONamespace>
        <oboInOwl:id>GAZ:00072045</oboInOwl:id>
        <rdfs:label>Municipality of Los Salias</rdfs:label>
    </owl:NamedIndividual>
    


    <!-- http://purl.obolibrary.org/obo/GAZ_00072046 -->

    <owl:NamedIndividual rdf:about="http://purl.obolibrary.org/obo/GAZ_00072046">
        <obo:RO_0001025 rdf:resource="http://purl.obolibrary.org/obo/GAZ_00011620"/>
        <oboInOwl:hasOBONamespace>GAZ</oboInOwl:hasOBONamespace>
        <oboInOwl:id>GAZ:00072046</oboInOwl:id>
        <rdfs:label>Municipality of Acosta</rdfs:label>
    </owl:NamedIndividual>
    


    <!-- http://purl.obolibrary.org/obo/GAZ_00072047 -->

    <owl:NamedIndividual rdf:about="http://purl.obolibrary.org/obo/GAZ_00072047">
        <obo:RO_0001025 rdf:resource="http://purl.obolibrary.org/obo/GAZ_00011620"/>
        <oboInOwl:hasOBONamespace>GAZ</oboInOwl:hasOBONamespace>
        <oboInOwl:id>GAZ:00072047</oboInOwl:id>
        <rdfs:label>Municipality of Cedeno</rdfs:label>
    </owl:NamedIndividual>
    


    <!-- http://purl.obolibrary.org/obo/GAZ_00072048 -->

    <owl:NamedIndividual rdf:about="http://purl.obolibrary.org/obo/GAZ_00072048">
        <obo:RO_0001025 rdf:resource="http://purl.obolibrary.org/obo/GAZ_00011620"/>
        <oboInOwl:hasOBONamespace>GAZ</oboInOwl:hasOBONamespace>
        <oboInOwl:id>GAZ:00072048</oboInOwl:id>
        <rdfs:label>Municipality of Caripe</rdfs:label>
    </owl:NamedIndividual>
    


    <!-- http://purl.obolibrary.org/obo/GAZ_00072049 -->

    <owl:NamedIndividual rdf:about="http://purl.obolibrary.org/obo/GAZ_00072049">
        <obo:RO_0001025 rdf:resource="http://purl.obolibrary.org/obo/GAZ_00011620"/>
        <oboInOwl:hasOBONamespace>GAZ</oboInOwl:hasOBONamespace>
        <oboInOwl:id>GAZ:00072049</oboInOwl:id>
        <rdfs:label>Municipality of Bolivar</rdfs:label>
    </owl:NamedIndividual>
    


    <!-- http://purl.obolibrary.org/obo/GAZ_00072050 -->

    <owl:NamedIndividual rdf:about="http://purl.obolibrary.org/obo/GAZ_00072050">
        <obo:RO_0001025 rdf:resource="http://purl.obolibrary.org/obo/GAZ_00011620"/>
        <oboInOwl:hasOBONamespace>GAZ</oboInOwl:hasOBONamespace>
        <oboInOwl:id>GAZ:00072050</oboInOwl:id>
        <rdfs:label>Municipality of Piar</rdfs:label>
    </owl:NamedIndividual>
    


    <!-- http://purl.obolibrary.org/obo/GAZ_00072051 -->

    <owl:NamedIndividual rdf:about="http://purl.obolibrary.org/obo/GAZ_00072051">
        <obo:RO_0001025 rdf:resource="http://purl.obolibrary.org/obo/GAZ_00011620"/>
        <oboInOwl:hasOBONamespace>GAZ</oboInOwl:hasOBONamespace>
        <oboInOwl:id>GAZ:00072051</oboInOwl:id>
        <rdfs:label>Municipality of Libertador</rdfs:label>
    </owl:NamedIndividual>
    


    <!-- http://purl.obolibrary.org/obo/GAZ_00072052 -->

    <owl:NamedIndividual rdf:about="http://purl.obolibrary.org/obo/GAZ_00072052">
        <obo:RO_0001025 rdf:resource="http://purl.obolibrary.org/obo/GAZ_00011620"/>
        <oboInOwl:hasOBONamespace>GAZ</oboInOwl:hasOBONamespace>
        <oboInOwl:id>GAZ:00072052</oboInOwl:id>
        <rdfs:label>Municipality of Uracoa</rdfs:label>
    </owl:NamedIndividual>
    


    <!-- http://purl.obolibrary.org/obo/GAZ_00072053 -->

    <owl:NamedIndividual rdf:about="http://purl.obolibrary.org/obo/GAZ_00072053">
        <obo:RO_0001025 rdf:resource="http://purl.obolibrary.org/obo/GAZ_00011620"/>
        <oboInOwl:hasOBONamespace>GAZ</oboInOwl:hasOBONamespace>
        <oboInOwl:id>GAZ:00072053</oboInOwl:id>
        <rdfs:label>Municipality of Punceres</rdfs:label>
    </owl:NamedIndividual>
    


    <!-- http://purl.obolibrary.org/obo/GAZ_00072054 -->

    <owl:NamedIndividual rdf:about="http://purl.obolibrary.org/obo/GAZ_00072054">
        <obo:RO_0001025 rdf:resource="http://purl.obolibrary.org/obo/GAZ_00011620"/>
        <oboInOwl:hasOBONamespace>GAZ</oboInOwl:hasOBONamespace>
        <oboInOwl:id>GAZ:00072054</oboInOwl:id>
        <rdfs:label>Municipality of Sotillo</rdfs:label>
    </owl:NamedIndividual>
    


    <!-- http://purl.obolibrary.org/obo/GAZ_00072055 -->

    <owl:NamedIndividual rdf:about="http://purl.obolibrary.org/obo/GAZ_00072055">
        <obo:RO_0001025 rdf:resource="http://purl.obolibrary.org/obo/GAZ_00011620"/>
        <oboInOwl:hasOBONamespace>GAZ</oboInOwl:hasOBONamespace>
        <oboInOwl:id>GAZ:00072055</oboInOwl:id>
        <rdfs:label>Municipality of Ezequiel Zamora</rdfs:label>
    </owl:NamedIndividual>
    


    <!-- http://purl.obolibrary.org/obo/GAZ_00072056 -->

    <owl:NamedIndividual rdf:about="http://purl.obolibrary.org/obo/GAZ_00072056">
        <obo:RO_0001025 rdf:resource="http://purl.obolibrary.org/obo/GAZ_00011620"/>
        <oboInOwl:hasOBONamespace>GAZ</oboInOwl:hasOBONamespace>
        <oboInOwl:id>GAZ:00072056</oboInOwl:id>
        <rdfs:label>Municipality of Maturin</rdfs:label>
    </owl:NamedIndividual>
    


    <!-- http://purl.obolibrary.org/obo/GAZ_00072057 -->

    <owl:NamedIndividual rdf:about="http://purl.obolibrary.org/obo/GAZ_00072057">
        <obo:RO_0001025 rdf:resource="http://purl.obolibrary.org/obo/GAZ_00011620"/>
        <oboInOwl:hasOBONamespace>GAZ</oboInOwl:hasOBONamespace>
        <oboInOwl:id>GAZ:00072057</oboInOwl:id>
        <rdfs:label>Municipality of Santa Barbara</rdfs:label>
    </owl:NamedIndividual>
    


    <!-- http://purl.obolibrary.org/obo/GAZ_00072058 -->

    <owl:NamedIndividual rdf:about="http://purl.obolibrary.org/obo/GAZ_00072058">
        <obo:RO_0001025 rdf:resource="http://purl.obolibrary.org/obo/GAZ_00011620"/>
        <oboInOwl:hasOBONamespace>GAZ</oboInOwl:hasOBONamespace>
        <oboInOwl:id>GAZ:00072058</oboInOwl:id>
        <rdfs:label>Municipality of Aguasay</rdfs:label>
    </owl:NamedIndividual>
    


    <!-- http://purl.obolibrary.org/obo/GAZ_00072059 -->

    <owl:NamedIndividual rdf:about="http://purl.obolibrary.org/obo/GAZ_00072059">
        <obo:RO_0001025 rdf:resource="http://purl.obolibrary.org/obo/GAZ_00011627"/>
        <oboInOwl:hasOBONamespace>GAZ</oboInOwl:hasOBONamespace>
        <oboInOwl:id>GAZ:00072059</oboInOwl:id>
        <rdfs:label>Municipality of Garcia</rdfs:label>
    </owl:NamedIndividual>
    


    <!-- http://purl.obolibrary.org/obo/GAZ_00072060 -->

    <owl:NamedIndividual rdf:about="http://purl.obolibrary.org/obo/GAZ_00072060">
        <obo:RO_0001025 rdf:resource="http://purl.obolibrary.org/obo/GAZ_00011627"/>
        <oboInOwl:hasOBONamespace>GAZ</oboInOwl:hasOBONamespace>
        <oboInOwl:id>GAZ:00072060</oboInOwl:id>
        <rdfs:label>Municipality of Marcano</rdfs:label>
    </owl:NamedIndividual>
    


    <!-- http://purl.obolibrary.org/obo/GAZ_00072061 -->

    <owl:NamedIndividual rdf:about="http://purl.obolibrary.org/obo/GAZ_00072061">
        <obo:RO_0001025 rdf:resource="http://purl.obolibrary.org/obo/GAZ_00011627"/>
        <oboInOwl:hasOBONamespace>GAZ</oboInOwl:hasOBONamespace>
        <oboInOwl:id>GAZ:00072061</oboInOwl:id>
        <rdfs:label>Municipality of Villalba</rdfs:label>
    </owl:NamedIndividual>
    


    <!-- http://purl.obolibrary.org/obo/GAZ_00072062 -->

    <owl:NamedIndividual rdf:about="http://purl.obolibrary.org/obo/GAZ_00072062">
        <obo:RO_0001025 rdf:resource="http://purl.obolibrary.org/obo/GAZ_00011627"/>
        <oboInOwl:hasOBONamespace>GAZ</oboInOwl:hasOBONamespace>
        <oboInOwl:id>GAZ:00072062</oboInOwl:id>
        <rdfs:label>Municipality of Maneiro</rdfs:label>
    </owl:NamedIndividual>
    


    <!-- http://purl.obolibrary.org/obo/GAZ_00072063 -->

    <owl:NamedIndividual rdf:about="http://purl.obolibrary.org/obo/GAZ_00072063">
        <obo:RO_0001025 rdf:resource="http://purl.obolibrary.org/obo/GAZ_00011627"/>
        <oboInOwl:hasOBONamespace>GAZ</oboInOwl:hasOBONamespace>
        <oboInOwl:id>GAZ:00072063</oboInOwl:id>
        <rdfs:label>Municipality of Antolin del Campo</rdfs:label>
    </owl:NamedIndividual>
    


    <!-- http://purl.obolibrary.org/obo/GAZ_00072064 -->

    <owl:NamedIndividual rdf:about="http://purl.obolibrary.org/obo/GAZ_00072064">
        <obo:RO_0001025 rdf:resource="http://purl.obolibrary.org/obo/GAZ_00011627"/>
        <oboInOwl:hasOBONamespace>GAZ</oboInOwl:hasOBONamespace>
        <oboInOwl:id>GAZ:00072064</oboInOwl:id>
        <rdfs:label>Peninsula de Macanao</rdfs:label>
    </owl:NamedIndividual>
    


    <!-- http://purl.obolibrary.org/obo/GAZ_00072065 -->

    <owl:NamedIndividual rdf:about="http://purl.obolibrary.org/obo/GAZ_00072065">
        <obo:RO_0001025 rdf:resource="http://purl.obolibrary.org/obo/GAZ_00011627"/>
        <oboInOwl:hasOBONamespace>GAZ</oboInOwl:hasOBONamespace>
        <oboInOwl:id>GAZ:00072065</oboInOwl:id>
        <rdfs:label>Municipality of Gomez</rdfs:label>
    </owl:NamedIndividual>
    


    <!-- http://purl.obolibrary.org/obo/GAZ_00072066 -->

    <owl:NamedIndividual rdf:about="http://purl.obolibrary.org/obo/GAZ_00072066">
        <obo:RO_0001025 rdf:resource="http://purl.obolibrary.org/obo/GAZ_00011627"/>
        <oboInOwl:hasOBONamespace>GAZ</oboInOwl:hasOBONamespace>
        <oboInOwl:id>GAZ:00072066</oboInOwl:id>
        <rdfs:label>Municipality of Diaz</rdfs:label>
    </owl:NamedIndividual>
    


    <!-- http://purl.obolibrary.org/obo/GAZ_00072067 -->

    <owl:NamedIndividual rdf:about="http://purl.obolibrary.org/obo/GAZ_00072067">
        <obo:RO_0001025 rdf:resource="http://purl.obolibrary.org/obo/GAZ_00011627"/>
        <oboInOwl:hasOBONamespace>GAZ</oboInOwl:hasOBONamespace>
        <oboInOwl:id>GAZ:00072067</oboInOwl:id>
        <rdfs:label>Municipality of Arismendi</rdfs:label>
    </owl:NamedIndividual>
    


    <!-- http://purl.obolibrary.org/obo/GAZ_00072068 -->

    <owl:NamedIndividual rdf:about="http://purl.obolibrary.org/obo/GAZ_00072068">
        <obo:RO_0001025 rdf:resource="http://purl.obolibrary.org/obo/GAZ_00011627"/>
        <oboInOwl:hasOBONamespace>GAZ</oboInOwl:hasOBONamespace>
        <oboInOwl:id>GAZ:00072068</oboInOwl:id>
        <rdfs:label>Municipality of Tubores</rdfs:label>
    </owl:NamedIndividual>
    


    <!-- http://purl.obolibrary.org/obo/GAZ_00072069 -->

    <owl:NamedIndividual rdf:about="http://purl.obolibrary.org/obo/GAZ_00072069">
        <obo:RO_0001025 rdf:resource="http://purl.obolibrary.org/obo/GAZ_00011627"/>
        <oboInOwl:hasOBONamespace>GAZ</oboInOwl:hasOBONamespace>
        <oboInOwl:id>GAZ:00072069</oboInOwl:id>
        <rdfs:label>Municipality of Marino</rdfs:label>
    </owl:NamedIndividual>
    


    <!-- http://purl.obolibrary.org/obo/GAZ_00072070 -->

    <owl:NamedIndividual rdf:about="http://purl.obolibrary.org/obo/GAZ_00072070">
        <obo:RO_0001025 rdf:resource="http://purl.obolibrary.org/obo/GAZ_00011598"/>
        <oboInOwl:hasOBONamespace>GAZ</oboInOwl:hasOBONamespace>
        <oboInOwl:id>GAZ:00072070</oboInOwl:id>
        <rdfs:label>Municipality of Agua Blanca</rdfs:label>
    </owl:NamedIndividual>
    


    <!-- http://purl.obolibrary.org/obo/GAZ_00072071 -->

    <owl:NamedIndividual rdf:about="http://purl.obolibrary.org/obo/GAZ_00072071">
        <obo:RO_0001025 rdf:resource="http://purl.obolibrary.org/obo/GAZ_00011598"/>
        <oboInOwl:hasOBONamespace>GAZ</oboInOwl:hasOBONamespace>
        <oboInOwl:id>GAZ:00072071</oboInOwl:id>
        <rdfs:label>Municipality of Araure</rdfs:label>
    </owl:NamedIndividual>
    


    <!-- http://purl.obolibrary.org/obo/GAZ_00072072 -->

    <owl:NamedIndividual rdf:about="http://purl.obolibrary.org/obo/GAZ_00072072">
        <obo:RO_0001025 rdf:resource="http://purl.obolibrary.org/obo/GAZ_00011598"/>
        <oboInOwl:hasOBONamespace>GAZ</oboInOwl:hasOBONamespace>
        <oboInOwl:id>GAZ:00072072</oboInOwl:id>
        <rdfs:label>Municipality of Paez</rdfs:label>
    </owl:NamedIndividual>
    


    <!-- http://purl.obolibrary.org/obo/GAZ_00072073 -->

    <owl:NamedIndividual rdf:about="http://purl.obolibrary.org/obo/GAZ_00072073">
        <obo:RO_0001025 rdf:resource="http://purl.obolibrary.org/obo/GAZ_00011598"/>
        <oboInOwl:hasOBONamespace>GAZ</oboInOwl:hasOBONamespace>
        <oboInOwl:id>GAZ:00072073</oboInOwl:id>
        <rdfs:label>Municipality of San Rafael de Onoto</rdfs:label>
    </owl:NamedIndividual>
    


    <!-- http://purl.obolibrary.org/obo/GAZ_00072074 -->

    <owl:NamedIndividual rdf:about="http://purl.obolibrary.org/obo/GAZ_00072074">
        <obo:RO_0001025 rdf:resource="http://purl.obolibrary.org/obo/GAZ_00011598"/>
        <oboInOwl:hasOBONamespace>GAZ</oboInOwl:hasOBONamespace>
        <oboInOwl:id>GAZ:00072074</oboInOwl:id>
        <rdfs:label>Municipality of Ospino</rdfs:label>
    </owl:NamedIndividual>
    


    <!-- http://purl.obolibrary.org/obo/GAZ_00072075 -->

    <owl:NamedIndividual rdf:about="http://purl.obolibrary.org/obo/GAZ_00072075">
        <obo:RO_0001025 rdf:resource="http://purl.obolibrary.org/obo/GAZ_00011598"/>
        <oboInOwl:hasOBONamespace>GAZ</oboInOwl:hasOBONamespace>
        <oboInOwl:id>GAZ:00072075</oboInOwl:id>
        <rdfs:label>Municipality of Sucre</rdfs:label>
    </owl:NamedIndividual>
    


    <!-- http://purl.obolibrary.org/obo/GAZ_00072076 -->

    <owl:NamedIndividual rdf:about="http://purl.obolibrary.org/obo/GAZ_00072076">
        <obo:RO_0001025 rdf:resource="http://purl.obolibrary.org/obo/GAZ_00011598"/>
        <oboInOwl:hasOBONamespace>GAZ</oboInOwl:hasOBONamespace>
        <oboInOwl:id>GAZ:00072076</oboInOwl:id>
        <rdfs:label>Municipality of Turen</rdfs:label>
    </owl:NamedIndividual>
    


    <!-- http://purl.obolibrary.org/obo/GAZ_00072077 -->

    <owl:NamedIndividual rdf:about="http://purl.obolibrary.org/obo/GAZ_00072077">
        <obo:RO_0001025 rdf:resource="http://purl.obolibrary.org/obo/GAZ_00011598"/>
        <oboInOwl:hasOBONamespace>GAZ</oboInOwl:hasOBONamespace>
        <oboInOwl:id>GAZ:00072077</oboInOwl:id>
        <rdfs:label>Municipality of San Genaro de Boconoito</rdfs:label>
    </owl:NamedIndividual>
    


    <!-- http://purl.obolibrary.org/obo/GAZ_00072078 -->

    <owl:NamedIndividual rdf:about="http://purl.obolibrary.org/obo/GAZ_00072078">
        <obo:RO_0001025 rdf:resource="http://purl.obolibrary.org/obo/GAZ_00011598"/>
        <oboInOwl:hasOBONamespace>GAZ</oboInOwl:hasOBONamespace>
        <oboInOwl:id>GAZ:00072078</oboInOwl:id>
        <rdfs:label>Municipality of Papelon</rdfs:label>
    </owl:NamedIndividual>
    


    <!-- http://purl.obolibrary.org/obo/GAZ_00072079 -->

    <owl:NamedIndividual rdf:about="http://purl.obolibrary.org/obo/GAZ_00072079">
        <obo:RO_0001025 rdf:resource="http://purl.obolibrary.org/obo/GAZ_00011598"/>
        <oboInOwl:hasOBONamespace>GAZ</oboInOwl:hasOBONamespace>
        <oboInOwl:id>GAZ:00072079</oboInOwl:id>
        <rdfs:label>Municipality of Santa Rosalia</rdfs:label>
    </owl:NamedIndividual>
    


    <!-- http://purl.obolibrary.org/obo/GAZ_00072080 -->

    <owl:NamedIndividual rdf:about="http://purl.obolibrary.org/obo/GAZ_00072080">
        <obo:RO_0001025 rdf:resource="http://purl.obolibrary.org/obo/GAZ_00011598"/>
        <oboInOwl:hasOBONamespace>GAZ</oboInOwl:hasOBONamespace>
        <oboInOwl:id>GAZ:00072080</oboInOwl:id>
        <rdfs:label>Monsenor Jose Vicente de Unda</rdfs:label>
    </owl:NamedIndividual>
    


    <!-- http://purl.obolibrary.org/obo/GAZ_00072081 -->

    <owl:NamedIndividual rdf:about="http://purl.obolibrary.org/obo/GAZ_00072081">
        <obo:RO_0001025 rdf:resource="http://purl.obolibrary.org/obo/GAZ_00011626"/>
        <oboInOwl:hasOBONamespace>GAZ</oboInOwl:hasOBONamespace>
        <oboInOwl:id>GAZ:00072081</oboInOwl:id>
        <rdfs:label>Municipality of Andres Mata</rdfs:label>
    </owl:NamedIndividual>
    


    <!-- http://purl.obolibrary.org/obo/GAZ_00072082 -->

    <owl:NamedIndividual rdf:about="http://purl.obolibrary.org/obo/GAZ_00072082">
        <obo:RO_0001025 rdf:resource="http://purl.obolibrary.org/obo/GAZ_00011626"/>
        <oboInOwl:hasOBONamespace>GAZ</oboInOwl:hasOBONamespace>
        <oboInOwl:id>GAZ:00072082</oboInOwl:id>
        <rdfs:label>Municipality of Cruz Salmeron Acosta</rdfs:label>
    </owl:NamedIndividual>
    


    <!-- http://purl.obolibrary.org/obo/GAZ_00072083 -->

    <owl:NamedIndividual rdf:about="http://purl.obolibrary.org/obo/GAZ_00072083">
        <obo:RO_0001025 rdf:resource="http://purl.obolibrary.org/obo/GAZ_00011625"/>
        <oboInOwl:hasOBONamespace>GAZ</oboInOwl:hasOBONamespace>
        <oboInOwl:id>GAZ:00072083</oboInOwl:id>
        <rdfs:label>Municipality of Independencia</rdfs:label>
    </owl:NamedIndividual>
    


    <!-- http://purl.obolibrary.org/obo/GAZ_00072084 -->

    <owl:NamedIndividual rdf:about="http://purl.obolibrary.org/obo/GAZ_00072084">
        <obo:RO_0001025 rdf:resource="http://purl.obolibrary.org/obo/GAZ_00011626"/>
        <oboInOwl:hasOBONamespace>GAZ</oboInOwl:hasOBONamespace>
        <oboInOwl:id>GAZ:00072084</oboInOwl:id>
        <rdfs:label>Municipality of Marino</rdfs:label>
    </owl:NamedIndividual>
    


    <!-- http://purl.obolibrary.org/obo/GAZ_00072085 -->

    <owl:NamedIndividual rdf:about="http://purl.obolibrary.org/obo/GAZ_00072085">
        <obo:RO_0001025 rdf:resource="http://purl.obolibrary.org/obo/GAZ_00011626"/>
        <oboInOwl:hasOBONamespace>GAZ</oboInOwl:hasOBONamespace>
        <oboInOwl:id>GAZ:00072085</oboInOwl:id>
        <rdfs:label>Municipality of Andres Eloy Blanco</rdfs:label>
    </owl:NamedIndividual>
    


    <!-- http://purl.obolibrary.org/obo/GAZ_00072086 -->

    <owl:NamedIndividual rdf:about="http://purl.obolibrary.org/obo/GAZ_00072086">
        <obo:RO_0001025 rdf:resource="http://purl.obolibrary.org/obo/GAZ_00011626"/>
        <oboInOwl:hasOBONamespace>GAZ</oboInOwl:hasOBONamespace>
        <oboInOwl:id>GAZ:00072086</oboInOwl:id>
        <rdfs:label>Municipality of Bolivar</rdfs:label>
    </owl:NamedIndividual>
    


    <!-- http://purl.obolibrary.org/obo/GAZ_00072087 -->

    <owl:NamedIndividual rdf:about="http://purl.obolibrary.org/obo/GAZ_00072087">
        <obo:RO_0001025 rdf:resource="http://purl.obolibrary.org/obo/GAZ_00011625"/>
        <oboInOwl:hasOBONamespace>GAZ</oboInOwl:hasOBONamespace>
        <oboInOwl:id>GAZ:00072087</oboInOwl:id>
        <rdfs:label>Municipality of Libertador</rdfs:label>
    </owl:NamedIndividual>
    


    <!-- http://purl.obolibrary.org/obo/GAZ_00072088 -->

    <owl:NamedIndividual rdf:about="http://purl.obolibrary.org/obo/GAZ_00072088">
        <obo:RO_0001025 rdf:resource="http://purl.obolibrary.org/obo/GAZ_00011626"/>
        <oboInOwl:hasOBONamespace>GAZ</oboInOwl:hasOBONamespace>
        <oboInOwl:id>GAZ:00072088</oboInOwl:id>
        <rdfs:label>Municipality of Ribero</rdfs:label>
    </owl:NamedIndividual>
    


    <!-- http://purl.obolibrary.org/obo/GAZ_00072089 -->

    <owl:NamedIndividual rdf:about="http://purl.obolibrary.org/obo/GAZ_00072089">
        <obo:RO_0001025 rdf:resource="http://purl.obolibrary.org/obo/GAZ_00011626"/>
        <oboInOwl:hasOBONamespace>GAZ</oboInOwl:hasOBONamespace>
        <oboInOwl:id>GAZ:00072089</oboInOwl:id>
        <rdfs:label>Municipality of Arismendi</rdfs:label>
    </owl:NamedIndividual>
    


    <!-- http://purl.obolibrary.org/obo/GAZ_00072090 -->

    <owl:NamedIndividual rdf:about="http://purl.obolibrary.org/obo/GAZ_00072090">
        <obo:RO_0001025 rdf:resource="http://purl.obolibrary.org/obo/GAZ_00011626"/>
        <oboInOwl:hasOBONamespace>GAZ</oboInOwl:hasOBONamespace>
        <oboInOwl:id>GAZ:00072090</oboInOwl:id>
        <rdfs:label>Municipality of Mejia</rdfs:label>
    </owl:NamedIndividual>
    


    <!-- http://purl.obolibrary.org/obo/GAZ_00072091 -->

    <owl:NamedIndividual rdf:about="http://purl.obolibrary.org/obo/GAZ_00072091">
        <obo:RO_0001025 rdf:resource="http://purl.obolibrary.org/obo/GAZ_00011625"/>
        <oboInOwl:hasOBONamespace>GAZ</oboInOwl:hasOBONamespace>
        <oboInOwl:id>GAZ:00072091</oboInOwl:id>
        <rdfs:label>Municipality of Lobatera</rdfs:label>
    </owl:NamedIndividual>
    


    <!-- http://purl.obolibrary.org/obo/GAZ_00072092 -->

    <owl:NamedIndividual rdf:about="http://purl.obolibrary.org/obo/GAZ_00072092">
        <obo:RO_0001025 rdf:resource="http://purl.obolibrary.org/obo/GAZ_00011626"/>
        <oboInOwl:hasOBONamespace>GAZ</oboInOwl:hasOBONamespace>
        <oboInOwl:id>GAZ:00072092</oboInOwl:id>
        <rdfs:label>Municipality of Cajigal</rdfs:label>
    </owl:NamedIndividual>
    


    <!-- http://purl.obolibrary.org/obo/GAZ_00072093 -->

    <owl:NamedIndividual rdf:about="http://purl.obolibrary.org/obo/GAZ_00072093">
        <obo:RO_0001025 rdf:resource="http://purl.obolibrary.org/obo/GAZ_00011626"/>
        <oboInOwl:hasOBONamespace>GAZ</oboInOwl:hasOBONamespace>
        <oboInOwl:id>GAZ:00072093</oboInOwl:id>
        <rdfs:label>Municipality of Bermudez</rdfs:label>
    </owl:NamedIndividual>
    


    <!-- http://purl.obolibrary.org/obo/GAZ_00072094 -->

    <owl:NamedIndividual rdf:about="http://purl.obolibrary.org/obo/GAZ_00072094">
        <obo:RO_0001025 rdf:resource="http://purl.obolibrary.org/obo/GAZ_00011626"/>
        <oboInOwl:hasOBONamespace>GAZ</oboInOwl:hasOBONamespace>
        <oboInOwl:id>GAZ:00072094</oboInOwl:id>
        <rdfs:label>Municipality of Sucre</rdfs:label>
    </owl:NamedIndividual>
    


    <!-- http://purl.obolibrary.org/obo/GAZ_00072095 -->

    <owl:NamedIndividual rdf:about="http://purl.obolibrary.org/obo/GAZ_00072095">
        <obo:RO_0001025 rdf:resource="http://purl.obolibrary.org/obo/GAZ_00011626"/>
        <oboInOwl:hasOBONamespace>GAZ</oboInOwl:hasOBONamespace>
        <oboInOwl:id>GAZ:00072095</oboInOwl:id>
        <rdfs:label>Municipality of Benitez</rdfs:label>
    </owl:NamedIndividual>
    


    <!-- http://purl.obolibrary.org/obo/GAZ_00072096 -->

    <owl:NamedIndividual rdf:about="http://purl.obolibrary.org/obo/GAZ_00072096">
        <obo:RO_0001025 rdf:resource="http://purl.obolibrary.org/obo/GAZ_00011626"/>
        <oboInOwl:hasOBONamespace>GAZ</oboInOwl:hasOBONamespace>
        <oboInOwl:id>GAZ:00072096</oboInOwl:id>
        <rdfs:label>Municipality of Valdez</rdfs:label>
    </owl:NamedIndividual>
    


    <!-- http://purl.obolibrary.org/obo/GAZ_00072097 -->

    <owl:NamedIndividual rdf:about="http://purl.obolibrary.org/obo/GAZ_00072097">
        <obo:RO_0001025 rdf:resource="http://purl.obolibrary.org/obo/GAZ_00011626"/>
        <oboInOwl:hasOBONamespace>GAZ</oboInOwl:hasOBONamespace>
        <oboInOwl:id>GAZ:00072097</oboInOwl:id>
        <rdfs:label>Municipality of Montes</rdfs:label>
    </owl:NamedIndividual>
    


    <!-- http://purl.obolibrary.org/obo/GAZ_00072098 -->

    <owl:NamedIndividual rdf:about="http://purl.obolibrary.org/obo/GAZ_00072098">
        <obo:RO_0001025 rdf:resource="http://purl.obolibrary.org/obo/GAZ_00011626"/>
        <oboInOwl:hasOBONamespace>GAZ</oboInOwl:hasOBONamespace>
        <oboInOwl:id>GAZ:00072098</oboInOwl:id>
        <rdfs:label>Municipality of Libertador</rdfs:label>
    </owl:NamedIndividual>
    


    <!-- http://purl.obolibrary.org/obo/GAZ_00072099 -->

    <owl:NamedIndividual rdf:about="http://purl.obolibrary.org/obo/GAZ_00072099">
        <obo:RO_0001025 rdf:resource="http://purl.obolibrary.org/obo/GAZ_00011625"/>
        <oboInOwl:hasOBONamespace>GAZ</oboInOwl:hasOBONamespace>
        <oboInOwl:id>GAZ:00072099</oboInOwl:id>
        <rdfs:label>Municipality of Michelena</rdfs:label>
    </owl:NamedIndividual>
    


    <!-- http://purl.obolibrary.org/obo/GAZ_00072100 -->

    <owl:NamedIndividual rdf:about="http://purl.obolibrary.org/obo/GAZ_00072100">
        <obo:RO_0001025 rdf:resource="http://purl.obolibrary.org/obo/GAZ_00011625"/>
        <oboInOwl:hasOBONamespace>GAZ</oboInOwl:hasOBONamespace>
        <oboInOwl:id>GAZ:00072100</oboInOwl:id>
        <rdfs:label>Municipality of Jose Maria Vargas</rdfs:label>
    </owl:NamedIndividual>
    


    <!-- http://purl.obolibrary.org/obo/GAZ_00072101 -->

    <owl:NamedIndividual rdf:about="http://purl.obolibrary.org/obo/GAZ_00072101">
        <obo:RO_0001025 rdf:resource="http://purl.obolibrary.org/obo/GAZ_00011625"/>
        <oboInOwl:hasOBONamespace>GAZ</oboInOwl:hasOBONamespace>
        <oboInOwl:id>GAZ:00072101</oboInOwl:id>
        <rdfs:label>Municipality of Samuel Dario Maldonado</rdfs:label>
    </owl:NamedIndividual>
    


    <!-- http://purl.obolibrary.org/obo/GAZ_00072102 -->

    <owl:NamedIndividual rdf:about="http://purl.obolibrary.org/obo/GAZ_00072102">
        <obo:RO_0001025 rdf:resource="http://purl.obolibrary.org/obo/GAZ_00011625"/>
        <oboInOwl:hasOBONamespace>GAZ</oboInOwl:hasOBONamespace>
        <oboInOwl:id>GAZ:00072102</oboInOwl:id>
        <rdfs:label>Municipality of Francisco de Miranda</rdfs:label>
    </owl:NamedIndividual>
    


    <!-- http://purl.obolibrary.org/obo/GAZ_00072103 -->

    <owl:NamedIndividual rdf:about="http://purl.obolibrary.org/obo/GAZ_00072103">
        <obo:RO_0001025 rdf:resource="http://purl.obolibrary.org/obo/GAZ_00011625"/>
        <oboInOwl:hasOBONamespace>GAZ</oboInOwl:hasOBONamespace>
        <oboInOwl:id>GAZ:00072103</oboInOwl:id>
        <rdfs:label>Municipality of Panamericano</rdfs:label>
    </owl:NamedIndividual>
    


    <!-- http://purl.obolibrary.org/obo/GAZ_00072104 -->

    <owl:NamedIndividual rdf:about="http://purl.obolibrary.org/obo/GAZ_00072104">
        <obo:RO_0001025 rdf:resource="http://purl.obolibrary.org/obo/GAZ_00011625"/>
        <oboInOwl:hasOBONamespace>GAZ</oboInOwl:hasOBONamespace>
        <oboInOwl:id>GAZ:00072104</oboInOwl:id>
        <rdfs:label>Municipality of Junin</rdfs:label>
    </owl:NamedIndividual>
    


    <!-- http://purl.obolibrary.org/obo/GAZ_00072105 -->

    <owl:NamedIndividual rdf:about="http://purl.obolibrary.org/obo/GAZ_00072105">
        <obo:RO_0001025 rdf:resource="http://purl.obolibrary.org/obo/GAZ_00011625"/>
        <oboInOwl:hasOBONamespace>GAZ</oboInOwl:hasOBONamespace>
        <oboInOwl:id>GAZ:00072105</oboInOwl:id>
        <rdfs:label>Municipality of San Judas Tadeo</rdfs:label>
    </owl:NamedIndividual>
    


    <!-- http://purl.obolibrary.org/obo/GAZ_00072106 -->

    <owl:NamedIndividual rdf:about="http://purl.obolibrary.org/obo/GAZ_00072106">
        <obo:RO_0001025 rdf:resource="http://purl.obolibrary.org/obo/GAZ_00011625"/>
        <oboInOwl:hasOBONamespace>GAZ</oboInOwl:hasOBONamespace>
        <oboInOwl:id>GAZ:00072106</oboInOwl:id>
        <rdfs:label>Municipality of Fernandez Feo</rdfs:label>
    </owl:NamedIndividual>
    


    <!-- http://purl.obolibrary.org/obo/GAZ_00072107 -->

    <owl:NamedIndividual rdf:about="http://purl.obolibrary.org/obo/GAZ_00072107">
        <obo:RO_0001025 rdf:resource="http://purl.obolibrary.org/obo/GAZ_00011625"/>
        <oboInOwl:hasOBONamespace>GAZ</oboInOwl:hasOBONamespace>
        <oboInOwl:id>GAZ:00072107</oboInOwl:id>
        <rdfs:label>Municipality of Pedro Maria Urena</rdfs:label>
    </owl:NamedIndividual>
    


    <!-- http://purl.obolibrary.org/obo/GAZ_00072108 -->

    <owl:NamedIndividual rdf:about="http://purl.obolibrary.org/obo/GAZ_00072108">
        <obo:RO_0001025 rdf:resource="http://purl.obolibrary.org/obo/GAZ_00011625"/>
        <oboInOwl:hasOBONamespace>GAZ</oboInOwl:hasOBONamespace>
        <oboInOwl:id>GAZ:00072108</oboInOwl:id>
        <rdfs:label>Municipality of Guasimos</rdfs:label>
    </owl:NamedIndividual>
    


    <!-- http://purl.obolibrary.org/obo/GAZ_00072109 -->

    <owl:NamedIndividual rdf:about="http://purl.obolibrary.org/obo/GAZ_00072109">
        <obo:RO_0001025 rdf:resource="http://purl.obolibrary.org/obo/GAZ_00011625"/>
        <oboInOwl:hasOBONamespace>GAZ</oboInOwl:hasOBONamespace>
        <oboInOwl:id>GAZ:00072109</oboInOwl:id>
        <rdfs:label>Municipality of San Cristobal</rdfs:label>
    </owl:NamedIndividual>
    


    <!-- http://purl.obolibrary.org/obo/GAZ_00072110 -->

    <owl:NamedIndividual rdf:about="http://purl.obolibrary.org/obo/GAZ_00072110">
        <obo:RO_0001025 rdf:resource="http://purl.obolibrary.org/obo/GAZ_00011625"/>
        <oboInOwl:hasOBONamespace>GAZ</oboInOwl:hasOBONamespace>
        <oboInOwl:id>GAZ:00072110</oboInOwl:id>
        <rdfs:label>Municipality of Cordoba</rdfs:label>
    </owl:NamedIndividual>
    


    <!-- http://purl.obolibrary.org/obo/GAZ_00072111 -->

    <owl:NamedIndividual rdf:about="http://purl.obolibrary.org/obo/GAZ_00072111">
        <obo:RO_0001025 rdf:resource="http://purl.obolibrary.org/obo/GAZ_00011625"/>
        <oboInOwl:hasOBONamespace>GAZ</oboInOwl:hasOBONamespace>
        <oboInOwl:id>GAZ:00072111</oboInOwl:id>
        <rdfs:label>Municipality of Simon Rodriguez</rdfs:label>
    </owl:NamedIndividual>
    


    <!-- http://purl.obolibrary.org/obo/GAZ_00072112 -->

    <owl:NamedIndividual rdf:about="http://purl.obolibrary.org/obo/GAZ_00072112">
        <obo:RO_0001025 rdf:resource="http://purl.obolibrary.org/obo/GAZ_00011625"/>
        <oboInOwl:hasOBONamespace>GAZ</oboInOwl:hasOBONamespace>
        <oboInOwl:id>GAZ:00072112</oboInOwl:id>
        <rdfs:label>Municipality of Libertad</rdfs:label>
    </owl:NamedIndividual>
    


    <!-- http://purl.obolibrary.org/obo/GAZ_00072113 -->

    <owl:NamedIndividual rdf:about="http://purl.obolibrary.org/obo/GAZ_00072113">
        <obo:RO_0001025 rdf:resource="http://purl.obolibrary.org/obo/GAZ_00011625"/>
        <oboInOwl:hasOBONamespace>GAZ</oboInOwl:hasOBONamespace>
        <oboInOwl:id>GAZ:00072113</oboInOwl:id>
        <rdfs:label>Municipality of Rafael Urdaneta</rdfs:label>
    </owl:NamedIndividual>
    


    <!-- http://purl.obolibrary.org/obo/GAZ_00072114 -->

    <owl:NamedIndividual rdf:about="http://purl.obolibrary.org/obo/GAZ_00072114">
        <obo:RO_0001025 rdf:resource="http://purl.obolibrary.org/obo/GAZ_00011625"/>
        <oboInOwl:hasOBONamespace>GAZ</oboInOwl:hasOBONamespace>
        <oboInOwl:id>GAZ:00072114</oboInOwl:id>
        <rdfs:label>Municipality of Jauregui</rdfs:label>
    </owl:NamedIndividual>
    


    <!-- http://purl.obolibrary.org/obo/GAZ_00072115 -->

    <owl:NamedIndividual rdf:about="http://purl.obolibrary.org/obo/GAZ_00072115">
        <obo:RO_0001025 rdf:resource="http://purl.obolibrary.org/obo/GAZ_00011625"/>
        <oboInOwl:hasOBONamespace>GAZ</oboInOwl:hasOBONamespace>
        <oboInOwl:id>GAZ:00072115</oboInOwl:id>
        <rdfs:label>Municipality of Seboruco</rdfs:label>
    </owl:NamedIndividual>
    


    <!-- http://purl.obolibrary.org/obo/GAZ_00072116 -->

    <owl:NamedIndividual rdf:about="http://purl.obolibrary.org/obo/GAZ_00072116">
        <obo:RO_0001025 rdf:resource="http://purl.obolibrary.org/obo/GAZ_00011625"/>
        <oboInOwl:hasOBONamespace>GAZ</oboInOwl:hasOBONamespace>
        <oboInOwl:id>GAZ:00072116</oboInOwl:id>
        <rdfs:label>Municipality of Torbes</rdfs:label>
    </owl:NamedIndividual>
    


    <!-- http://purl.obolibrary.org/obo/GAZ_00072117 -->

    <owl:NamedIndividual rdf:about="http://purl.obolibrary.org/obo/GAZ_00072117">
        <obo:RO_0001025 rdf:resource="http://purl.obolibrary.org/obo/GAZ_00011625"/>
        <oboInOwl:hasOBONamespace>GAZ</oboInOwl:hasOBONamespace>
        <oboInOwl:id>GAZ:00072117</oboInOwl:id>
        <rdfs:label>Municipality of Uribante</rdfs:label>
    </owl:NamedIndividual>
    


    <!-- http://purl.obolibrary.org/obo/GAZ_00072118 -->

    <owl:NamedIndividual rdf:about="http://purl.obolibrary.org/obo/GAZ_00072118">
        <obo:RO_0001025 rdf:resource="http://purl.obolibrary.org/obo/GAZ_00011625"/>
        <oboInOwl:hasOBONamespace>GAZ</oboInOwl:hasOBONamespace>
        <oboInOwl:id>GAZ:00072118</oboInOwl:id>
        <rdfs:label>Municipality of Garcia de Hevia</rdfs:label>
    </owl:NamedIndividual>
    


    <!-- http://purl.obolibrary.org/obo/GAZ_00072119 -->

    <owl:NamedIndividual rdf:about="http://purl.obolibrary.org/obo/GAZ_00072119">
        <obo:RO_0001025 rdf:resource="http://purl.obolibrary.org/obo/GAZ_00011625"/>
        <oboInOwl:hasOBONamespace>GAZ</oboInOwl:hasOBONamespace>
        <oboInOwl:id>GAZ:00072119</oboInOwl:id>
        <rdfs:label>Municipality of Sucre</rdfs:label>
    </owl:NamedIndividual>
    


    <!-- http://purl.obolibrary.org/obo/GAZ_00072120 -->

    <owl:NamedIndividual rdf:about="http://purl.obolibrary.org/obo/GAZ_00072120">
        <obo:RO_0001025 rdf:resource="http://purl.obolibrary.org/obo/GAZ_00011625"/>
        <oboInOwl:hasOBONamespace>GAZ</oboInOwl:hasOBONamespace>
        <oboInOwl:id>GAZ:00072120</oboInOwl:id>
        <rdfs:label>Municipality of Ayacucho</rdfs:label>
    </owl:NamedIndividual>
    


    <!-- http://purl.obolibrary.org/obo/GAZ_00072121 -->

    <owl:NamedIndividual rdf:about="http://purl.obolibrary.org/obo/GAZ_00072121">
        <obo:RO_0001025 rdf:resource="http://purl.obolibrary.org/obo/GAZ_00011625"/>
        <oboInOwl:hasOBONamespace>GAZ</oboInOwl:hasOBONamespace>
        <oboInOwl:id>GAZ:00072121</oboInOwl:id>
        <rdfs:label>Municipality of Andres Bello</rdfs:label>
    </owl:NamedIndividual>
    


    <!-- http://purl.obolibrary.org/obo/GAZ_00072122 -->

    <owl:NamedIndividual rdf:about="http://purl.obolibrary.org/obo/GAZ_00072122">
        <obo:RO_0001025 rdf:resource="http://purl.obolibrary.org/obo/GAZ_00011624"/>
        <oboInOwl:hasOBONamespace>GAZ</oboInOwl:hasOBONamespace>
        <oboInOwl:id>GAZ:00072122</oboInOwl:id>
        <rdfs:label>Municipality of Jose Felipe Marquez Canizales</rdfs:label>
    </owl:NamedIndividual>
    


    <!-- http://purl.obolibrary.org/obo/GAZ_00072123 -->

    <owl:NamedIndividual rdf:about="http://purl.obolibrary.org/obo/GAZ_00072123">
        <obo:RO_0001025 rdf:resource="http://purl.obolibrary.org/obo/GAZ_00011625"/>
        <oboInOwl:hasOBONamespace>GAZ</oboInOwl:hasOBONamespace>
        <oboInOwl:id>GAZ:00072123</oboInOwl:id>
        <rdfs:label>Municipality of Cardenas</rdfs:label>
    </owl:NamedIndividual>
    


    <!-- http://purl.obolibrary.org/obo/GAZ_00072124 -->

    <owl:NamedIndividual rdf:about="http://purl.obolibrary.org/obo/GAZ_00072124">
        <obo:RO_0001025 rdf:resource="http://purl.obolibrary.org/obo/GAZ_00011624"/>
        <oboInOwl:hasOBONamespace>GAZ</oboInOwl:hasOBONamespace>
        <oboInOwl:id>GAZ:00072124</oboInOwl:id>
        <rdfs:label>Municipality of Monte Carmelo</rdfs:label>
    </owl:NamedIndividual>
    


    <!-- http://purl.obolibrary.org/obo/GAZ_00072125 -->

    <owl:NamedIndividual rdf:about="http://purl.obolibrary.org/obo/GAZ_00072125">
        <obo:RO_0001025 rdf:resource="http://purl.obolibrary.org/obo/GAZ_00011625"/>
        <oboInOwl:hasOBONamespace>GAZ</oboInOwl:hasOBONamespace>
        <oboInOwl:id>GAZ:00072125</oboInOwl:id>
        <rdfs:label>Municipality of Bolivar</rdfs:label>
    </owl:NamedIndividual>
    


    <!-- http://purl.obolibrary.org/obo/GAZ_00072126 -->

    <owl:NamedIndividual rdf:about="http://purl.obolibrary.org/obo/GAZ_00072126">
        <obo:RO_0001025 rdf:resource="http://purl.obolibrary.org/obo/GAZ_00011624"/>
        <oboInOwl:hasOBONamespace>GAZ</oboInOwl:hasOBONamespace>
        <oboInOwl:id>GAZ:00072126</oboInOwl:id>
        <rdfs:label>Municipality of San Rafael de Carvajal</rdfs:label>
    </owl:NamedIndividual>
    


    <!-- http://purl.obolibrary.org/obo/GAZ_00072127 -->

    <owl:NamedIndividual rdf:about="http://purl.obolibrary.org/obo/GAZ_00072127">
        <obo:RO_0001025 rdf:resource="http://purl.obolibrary.org/obo/GAZ_00011625"/>
        <oboInOwl:hasOBONamespace>GAZ</oboInOwl:hasOBONamespace>
        <oboInOwl:id>GAZ:00072127</oboInOwl:id>
        <rdfs:label>Municipality of Antonio Romulo Costa</rdfs:label>
    </owl:NamedIndividual>
    


    <!-- http://purl.obolibrary.org/obo/GAZ_00072128 -->

    <owl:NamedIndividual rdf:about="http://purl.obolibrary.org/obo/GAZ_00072128">
        <obo:RO_0001025 rdf:resource="http://purl.obolibrary.org/obo/GAZ_00011624"/>
        <oboInOwl:hasOBONamespace>GAZ</oboInOwl:hasOBONamespace>
        <oboInOwl:id>GAZ:00072128</oboInOwl:id>
        <rdfs:label>Municipality of Rafael Rangel</rdfs:label>
    </owl:NamedIndividual>
    


    <!-- http://purl.obolibrary.org/obo/GAZ_00072129 -->

    <owl:NamedIndividual rdf:about="http://purl.obolibrary.org/obo/GAZ_00072129">
        <obo:RO_0001025 rdf:resource="http://purl.obolibrary.org/obo/GAZ_00011624"/>
        <oboInOwl:hasOBONamespace>GAZ</oboInOwl:hasOBONamespace>
        <oboInOwl:id>GAZ:00072129</oboInOwl:id>
        <rdfs:label>Municipality of Juan Vicente Campo Elias</rdfs:label>
    </owl:NamedIndividual>
    


    <!-- http://purl.obolibrary.org/obo/GAZ_00072130 -->

    <owl:NamedIndividual rdf:about="http://purl.obolibrary.org/obo/GAZ_00072130">
        <obo:RO_0001025 rdf:resource="http://purl.obolibrary.org/obo/GAZ_00011624"/>
        <oboInOwl:hasOBONamespace>GAZ</oboInOwl:hasOBONamespace>
        <oboInOwl:id>GAZ:00072130</oboInOwl:id>
        <rdfs:label>Municipality of Sucre</rdfs:label>
    </owl:NamedIndividual>
    


    <!-- http://purl.obolibrary.org/obo/GAZ_00072131 -->

    <owl:NamedIndividual rdf:about="http://purl.obolibrary.org/obo/GAZ_00072131">
        <obo:RO_0001025 rdf:resource="http://purl.obolibrary.org/obo/GAZ_00011624"/>
        <oboInOwl:hasOBONamespace>GAZ</oboInOwl:hasOBONamespace>
        <oboInOwl:id>GAZ:00072131</oboInOwl:id>
        <rdfs:label>Municipality of Carache</rdfs:label>
    </owl:NamedIndividual>
    


    <!-- http://purl.obolibrary.org/obo/GAZ_00072132 -->

    <owl:NamedIndividual rdf:about="http://purl.obolibrary.org/obo/GAZ_00072132">
        <obo:RO_0001025 rdf:resource="http://purl.obolibrary.org/obo/GAZ_00011624"/>
        <oboInOwl:hasOBONamespace>GAZ</oboInOwl:hasOBONamespace>
        <oboInOwl:id>GAZ:00072132</oboInOwl:id>
        <rdfs:label>Municipality of Motatan</rdfs:label>
    </owl:NamedIndividual>
    


    <!-- http://purl.obolibrary.org/obo/GAZ_00072133 -->

    <owl:NamedIndividual rdf:about="http://purl.obolibrary.org/obo/GAZ_00072133">
        <obo:RO_0001025 rdf:resource="http://purl.obolibrary.org/obo/GAZ_00011624"/>
        <oboInOwl:hasOBONamespace>GAZ</oboInOwl:hasOBONamespace>
        <oboInOwl:id>GAZ:00072133</oboInOwl:id>
        <rdfs:label>Municipality of Bolivar</rdfs:label>
    </owl:NamedIndividual>
    


    <!-- http://purl.obolibrary.org/obo/GAZ_00072134 -->

    <owl:NamedIndividual rdf:about="http://purl.obolibrary.org/obo/GAZ_00072134">
        <obo:RO_0001025 rdf:resource="http://purl.obolibrary.org/obo/GAZ_00011624"/>
        <oboInOwl:hasOBONamespace>GAZ</oboInOwl:hasOBONamespace>
        <oboInOwl:id>GAZ:00072134</oboInOwl:id>
        <rdfs:label>Municipality of Trujillo</rdfs:label>
    </owl:NamedIndividual>
    


    <!-- http://purl.obolibrary.org/obo/GAZ_00072135 -->

    <owl:NamedIndividual rdf:about="http://purl.obolibrary.org/obo/GAZ_00072135">
        <obo:RO_0001025 rdf:resource="http://purl.obolibrary.org/obo/GAZ_00011624"/>
        <oboInOwl:hasOBONamespace>GAZ</oboInOwl:hasOBONamespace>
        <oboInOwl:id>GAZ:00072135</oboInOwl:id>
        <rdfs:label>Municipality of Candelaria</rdfs:label>
    </owl:NamedIndividual>
    


    <!-- http://purl.obolibrary.org/obo/GAZ_00072136 -->

    <owl:NamedIndividual rdf:about="http://purl.obolibrary.org/obo/GAZ_00072136">
        <obo:RO_0001025 rdf:resource="http://purl.obolibrary.org/obo/GAZ_00011624"/>
        <oboInOwl:hasOBONamespace>GAZ</oboInOwl:hasOBONamespace>
        <oboInOwl:id>GAZ:00072136</oboInOwl:id>
        <rdfs:label>Municipality of Pampan</rdfs:label>
    </owl:NamedIndividual>
    


    <!-- http://purl.obolibrary.org/obo/GAZ_00072137 -->

    <owl:NamedIndividual rdf:about="http://purl.obolibrary.org/obo/GAZ_00072137">
        <obo:RO_0001025 rdf:resource="http://purl.obolibrary.org/obo/GAZ_00011624"/>
        <oboInOwl:hasOBONamespace>GAZ</oboInOwl:hasOBONamespace>
        <oboInOwl:id>GAZ:00072137</oboInOwl:id>
        <rdfs:label>Municipality of Escuque</rdfs:label>
    </owl:NamedIndividual>
    


    <!-- http://purl.obolibrary.org/obo/GAZ_00072138 -->

    <owl:NamedIndividual rdf:about="http://purl.obolibrary.org/obo/GAZ_00072138">
        <obo:RO_0001025 rdf:resource="http://purl.obolibrary.org/obo/GAZ_00011624"/>
        <oboInOwl:hasOBONamespace>GAZ</oboInOwl:hasOBONamespace>
        <oboInOwl:id>GAZ:00072138</oboInOwl:id>
        <rdfs:label>Municipality of Valera</rdfs:label>
    </owl:NamedIndividual>
    


    <!-- http://purl.obolibrary.org/obo/GAZ_00072139 -->

    <owl:NamedIndividual rdf:about="http://purl.obolibrary.org/obo/GAZ_00072139">
        <obo:RO_0001025 rdf:resource="http://purl.obolibrary.org/obo/GAZ_00011624"/>
        <oboInOwl:hasOBONamespace>GAZ</oboInOwl:hasOBONamespace>
        <oboInOwl:id>GAZ:00072139</oboInOwl:id>
        <rdfs:label>Municipality of Miranda</rdfs:label>
    </owl:NamedIndividual>
    


    <!-- http://purl.obolibrary.org/obo/GAZ_00072140 -->

    <owl:NamedIndividual rdf:about="http://purl.obolibrary.org/obo/GAZ_00072140">
        <obo:RO_0001025 rdf:resource="http://purl.obolibrary.org/obo/GAZ_00011624"/>
        <oboInOwl:hasOBONamespace>GAZ</oboInOwl:hasOBONamespace>
        <oboInOwl:id>GAZ:00072140</oboInOwl:id>
        <rdfs:label>Municipality of Bocono</rdfs:label>
    </owl:NamedIndividual>
    


    <!-- http://purl.obolibrary.org/obo/GAZ_00072141 -->

    <owl:NamedIndividual rdf:about="http://purl.obolibrary.org/obo/GAZ_00072141">
        <obo:RO_0001025 rdf:resource="http://purl.obolibrary.org/obo/GAZ_00011624"/>
        <oboInOwl:hasOBONamespace>GAZ</oboInOwl:hasOBONamespace>
        <oboInOwl:id>GAZ:00072141</oboInOwl:id>
        <rdfs:label>Municipality of La Ceiba</rdfs:label>
    </owl:NamedIndividual>
    


    <!-- http://purl.obolibrary.org/obo/GAZ_00072142 -->

    <owl:NamedIndividual rdf:about="http://purl.obolibrary.org/obo/GAZ_00072142">
        <obo:RO_0001025 rdf:resource="http://purl.obolibrary.org/obo/GAZ_00011624"/>
        <oboInOwl:hasOBONamespace>GAZ</oboInOwl:hasOBONamespace>
        <oboInOwl:id>GAZ:00072142</oboInOwl:id>
        <rdfs:label>Municipality of Urdaneta</rdfs:label>
    </owl:NamedIndividual>
    


    <!-- http://purl.obolibrary.org/obo/GAZ_00072143 -->

    <owl:NamedIndividual rdf:about="http://purl.obolibrary.org/obo/GAZ_00072143">
        <obo:RO_0001025 rdf:resource="http://purl.obolibrary.org/obo/GAZ_00011624"/>
        <oboInOwl:hasOBONamespace>GAZ</oboInOwl:hasOBONamespace>
        <oboInOwl:id>GAZ:00072143</oboInOwl:id>
        <rdfs:label>Municipality of Pampanito</rdfs:label>
    </owl:NamedIndividual>
    


    <!-- http://purl.obolibrary.org/obo/GAZ_00072144 -->

    <owl:NamedIndividual rdf:about="http://purl.obolibrary.org/obo/GAZ_00072144">
        <obo:RO_0001025 rdf:resource="http://purl.obolibrary.org/obo/GAZ_00011624"/>
        <oboInOwl:hasOBONamespace>GAZ</oboInOwl:hasOBONamespace>
        <oboInOwl:id>GAZ:00072144</oboInOwl:id>
        <rdfs:label>Municipality of Andres Bello</rdfs:label>
    </owl:NamedIndividual>
    


    <!-- http://purl.obolibrary.org/obo/GAZ_00072145 -->

    <owl:NamedIndividual rdf:about="http://purl.obolibrary.org/obo/GAZ_00072145">
        <obo:RO_0001025 rdf:resource="http://purl.obolibrary.org/obo/GAZ_00011629"/>
        <oboInOwl:hasOBONamespace>GAZ</oboInOwl:hasOBONamespace>
        <oboInOwl:id>GAZ:00072145</oboInOwl:id>
        <rdfs:label>Municipality of Vargas</rdfs:label>
    </owl:NamedIndividual>
    


    <!-- http://purl.obolibrary.org/obo/GAZ_00072146 -->

    <owl:NamedIndividual rdf:about="http://purl.obolibrary.org/obo/GAZ_00072146">
        <obo:RO_0001025 rdf:resource="http://purl.obolibrary.org/obo/GAZ_00011628"/>
        <oboInOwl:hasOBONamespace>GAZ</oboInOwl:hasOBONamespace>
        <oboInOwl:id>GAZ:00072146</oboInOwl:id>
        <rdfs:label>Municipality of Jose Antonio Paez</rdfs:label>
    </owl:NamedIndividual>
    


    <!-- http://purl.obolibrary.org/obo/GAZ_00072147 -->

    <owl:NamedIndividual rdf:about="http://purl.obolibrary.org/obo/GAZ_00072147">
        <obo:RO_0001025 rdf:resource="http://purl.obolibrary.org/obo/GAZ_00011628"/>
        <oboInOwl:hasOBONamespace>GAZ</oboInOwl:hasOBONamespace>
        <oboInOwl:id>GAZ:00072147</oboInOwl:id>
        <rdfs:label>Municipality of La Trinidad</rdfs:label>
    </owl:NamedIndividual>
    


    <!-- http://purl.obolibrary.org/obo/GAZ_00072148 -->

    <owl:NamedIndividual rdf:about="http://purl.obolibrary.org/obo/GAZ_00072148">
        <obo:RO_0001025 rdf:resource="http://purl.obolibrary.org/obo/GAZ_00011628"/>
        <oboInOwl:hasOBONamespace>GAZ</oboInOwl:hasOBONamespace>
        <oboInOwl:id>GAZ:00072148</oboInOwl:id>
        <rdfs:label>Municipality of Bruzual</rdfs:label>
    </owl:NamedIndividual>
    


    <!-- http://purl.obolibrary.org/obo/GAZ_00072149 -->

    <owl:NamedIndividual rdf:about="http://purl.obolibrary.org/obo/GAZ_00072149">
        <obo:RO_0001025 rdf:resource="http://purl.obolibrary.org/obo/GAZ_00011628"/>
        <oboInOwl:hasOBONamespace>GAZ</oboInOwl:hasOBONamespace>
        <oboInOwl:id>GAZ:00072149</oboInOwl:id>
        <rdfs:label>Municipality of Manuel</rdfs:label>
    </owl:NamedIndividual>
    


    <!-- http://purl.obolibrary.org/obo/GAZ_00072150 -->

    <owl:NamedIndividual rdf:about="http://purl.obolibrary.org/obo/GAZ_00072150">
        <obo:RO_0001025 rdf:resource="http://purl.obolibrary.org/obo/GAZ_00011628"/>
        <oboInOwl:hasOBONamespace>GAZ</oboInOwl:hasOBONamespace>
        <oboInOwl:id>GAZ:00072150</oboInOwl:id>
        <rdfs:label>Municipality of Bolivar</rdfs:label>
    </owl:NamedIndividual>
    


    <!-- http://purl.obolibrary.org/obo/GAZ_00072151 -->

    <owl:NamedIndividual rdf:about="http://purl.obolibrary.org/obo/GAZ_00072151">
        <obo:RO_0001025 rdf:resource="http://purl.obolibrary.org/obo/GAZ_00011628"/>
        <oboInOwl:hasOBONamespace>GAZ</oboInOwl:hasOBONamespace>
        <oboInOwl:id>GAZ:00072151</oboInOwl:id>
        <rdfs:label>Municipality of Independencia</rdfs:label>
    </owl:NamedIndividual>
    


    <!-- http://purl.obolibrary.org/obo/GAZ_00072152 -->

    <owl:NamedIndividual rdf:about="http://purl.obolibrary.org/obo/GAZ_00072152">
        <obo:RO_0001025 rdf:resource="http://purl.obolibrary.org/obo/GAZ_00011628"/>
        <oboInOwl:hasOBONamespace>GAZ</oboInOwl:hasOBONamespace>
        <oboInOwl:id>GAZ:00072152</oboInOwl:id>
        <rdfs:label>Municipality of Cocorote</rdfs:label>
    </owl:NamedIndividual>
    


    <!-- http://purl.obolibrary.org/obo/GAZ_00072153 -->

    <owl:NamedIndividual rdf:about="http://purl.obolibrary.org/obo/GAZ_00072153">
        <obo:RO_0001025 rdf:resource="http://purl.obolibrary.org/obo/GAZ_00011628"/>
        <oboInOwl:hasOBONamespace>GAZ</oboInOwl:hasOBONamespace>
        <oboInOwl:id>GAZ:00072153</oboInOwl:id>
        <rdfs:label>Municipality of San Felipe</rdfs:label>
    </owl:NamedIndividual>
    


    <!-- http://purl.obolibrary.org/obo/GAZ_00072154 -->

    <owl:NamedIndividual rdf:about="http://purl.obolibrary.org/obo/GAZ_00072154">
        <obo:RO_0001025 rdf:resource="http://purl.obolibrary.org/obo/GAZ_00011628"/>
        <oboInOwl:hasOBONamespace>GAZ</oboInOwl:hasOBONamespace>
        <oboInOwl:id>GAZ:00072154</oboInOwl:id>
        <rdfs:label>Municipality of Monge</rdfs:label>
    </owl:NamedIndividual>
    


    <!-- http://purl.obolibrary.org/obo/GAZ_00072155 -->

    <owl:NamedIndividual rdf:about="http://purl.obolibrary.org/obo/GAZ_00072155">
        <obo:RO_0001025 rdf:resource="http://purl.obolibrary.org/obo/GAZ_00011628"/>
        <oboInOwl:hasOBONamespace>GAZ</oboInOwl:hasOBONamespace>
        <oboInOwl:id>GAZ:00072155</oboInOwl:id>
        <rdfs:label>Municipality of Pena</rdfs:label>
    </owl:NamedIndividual>
    


    <!-- http://purl.obolibrary.org/obo/GAZ_00072156 -->

    <owl:NamedIndividual rdf:about="http://purl.obolibrary.org/obo/GAZ_00072156">
        <obo:RO_0001025 rdf:resource="http://purl.obolibrary.org/obo/GAZ_00011628"/>
        <oboInOwl:hasOBONamespace>GAZ</oboInOwl:hasOBONamespace>
        <oboInOwl:id>GAZ:00072156</oboInOwl:id>
        <rdfs:label>Municipality of Veroes</rdfs:label>
    </owl:NamedIndividual>
    


    <!-- http://purl.obolibrary.org/obo/GAZ_00072157 -->

    <owl:NamedIndividual rdf:about="http://purl.obolibrary.org/obo/GAZ_00072157">
        <obo:RO_0001025 rdf:resource="http://purl.obolibrary.org/obo/GAZ_00011628"/>
        <oboInOwl:hasOBONamespace>GAZ</oboInOwl:hasOBONamespace>
        <oboInOwl:id>GAZ:00072157</oboInOwl:id>
        <rdfs:label>Municipality of Aristides Bastidas</rdfs:label>
    </owl:NamedIndividual>
    


    <!-- http://purl.obolibrary.org/obo/GAZ_00072158 -->

    <owl:NamedIndividual rdf:about="http://purl.obolibrary.org/obo/GAZ_00072158">
        <obo:RO_0001025 rdf:resource="http://purl.obolibrary.org/obo/GAZ_00011628"/>
        <oboInOwl:hasOBONamespace>GAZ</oboInOwl:hasOBONamespace>
        <oboInOwl:id>GAZ:00072158</oboInOwl:id>
        <rdfs:label>Municipality of Sucre</rdfs:label>
    </owl:NamedIndividual>
    


    <!-- http://purl.obolibrary.org/obo/GAZ_00072159 -->

    <owl:NamedIndividual rdf:about="http://purl.obolibrary.org/obo/GAZ_00072159">
        <obo:RO_0001025 rdf:resource="http://purl.obolibrary.org/obo/GAZ_00011628"/>
        <oboInOwl:hasOBONamespace>GAZ</oboInOwl:hasOBONamespace>
        <oboInOwl:id>GAZ:00072159</oboInOwl:id>
        <rdfs:label>Municipality of Urachiche</rdfs:label>
    </owl:NamedIndividual>
    


    <!-- http://purl.obolibrary.org/obo/GAZ_00072160 -->

    <owl:NamedIndividual rdf:about="http://purl.obolibrary.org/obo/GAZ_00072160">
        <obo:RO_0001025 rdf:resource="http://purl.obolibrary.org/obo/GAZ_00011628"/>
        <oboInOwl:hasOBONamespace>GAZ</oboInOwl:hasOBONamespace>
        <oboInOwl:id>GAZ:00072160</oboInOwl:id>
        <rdfs:label>Municipality of Nirgua</rdfs:label>
    </owl:NamedIndividual>
    


    <!-- http://purl.obolibrary.org/obo/GAZ_00082192 -->

    <owl:NamedIndividual rdf:about="http://purl.obolibrary.org/obo/GAZ_00082192">
        <obo:RO_0001025 rdf:resource="http://purl.obolibrary.org/obo/GAZ_00047131"/>
        <obo:IAO_0000115>An island lying off the north coast of Ilha de Marajo in the delta lowlands at the mouth of the Amazon in the State of Para, Brazil.</obo:IAO_0000115>
        <oboInOwl:hasOBONamespace>GAZ</oboInOwl:hasOBONamespace>
        <oboInOwl:id>GAZ:00082192</oboInOwl:id>
        <rdfs:label>Ilha Caviana</rdfs:label>
    </owl:NamedIndividual>
    


    <!-- http://purl.obolibrary.org/obo/GAZ_00082193 -->

    <owl:NamedIndividual rdf:about="http://purl.obolibrary.org/obo/GAZ_00082193">
        <obo:RO_0001025 rdf:resource="http://purl.obolibrary.org/obo/GAZ_00047131"/>
        <obo:IAO_0000115>The second largest island of the River Amazon delta. It lies in the Brazilian State of Para, west of Marajo and near the confluence of the Amazon and the Xingu.</obo:IAO_0000115>
        <oboInOwl:hasOBONamespace>GAZ</oboInOwl:hasOBONamespace>
        <oboInOwl:id>GAZ:00082193</oboInOwl:id>
        <rdfs:label>Ilha Grande do Gurupa</rdfs:label>
    </owl:NamedIndividual>
    


    <!-- http://purl.obolibrary.org/obo/GAZ_00082204 -->

    <owl:NamedIndividual rdf:about="http://purl.obolibrary.org/obo/GAZ_00082204">
        <rdf:type rdf:resource="http://purl.obolibrary.org/obo/ENVO_00000423"/>
        <obo:RO_0001025 rdf:resource="http://purl.obolibrary.org/obo/GAZ_00047130"/>
        <obo:IAO_0000115>A fluvial island. It is bordered by four rivers: Amazon, Madeira, Sucunduri, and Abacaxis. It has been split into four completely separate parts by natural channels just like the one which isolates it from the mainland of America. So it is no longer one island, but indeed four islands. The total area of these islands sums up to 11,850 km2, making Ilha Tupinambarana the largest fluvial group of islands in the world.</obo:IAO_0000115>
        <oboInOwl:hasOBONamespace>GAZ</oboInOwl:hasOBONamespace>
        <oboInOwl:id>GAZ:00082204</oboInOwl:id>
        <rdfs:label>Tupinambarana</rdfs:label>
    </owl:NamedIndividual>
    


    <!-- http://purl.obolibrary.org/obo/GAZ_00082205 -->

    <owl:NamedIndividual rdf:about="http://purl.obolibrary.org/obo/GAZ_00082205">
        <obo:RO_0001025 rdf:resource="http://purl.obolibrary.org/obo/GAZ_00049223"/>
        <obo:IAO_0000115>An archipelago of about 400 fluvial islands.</obo:IAO_0000115>
        <oboInOwl:hasOBONamespace>GAZ</oboInOwl:hasOBONamespace>
        <oboInOwl:id>GAZ:00082205</oboInOwl:id>
        <rdfs:label>Anavilhanas</rdfs:label>
    </owl:NamedIndividual>
    


    <!-- http://purl.obolibrary.org/obo/GAZ_00082206 -->

    <owl:NamedIndividual rdf:about="http://purl.obolibrary.org/obo/GAZ_00082206">
        <obo:RO_0001025 rdf:resource="http://purl.obolibrary.org/obo/GAZ_00082205"/>
        <oboInOwl:hasOBONamespace>GAZ</oboInOwl:hasOBONamespace>
        <oboInOwl:id>GAZ:00082206</oboInOwl:id>
        <rdfs:label>Estacao Ecologica Anavilhanas</rdfs:label>
    </owl:NamedIndividual>
    


    <!-- http://purl.obolibrary.org/obo/GAZ_00089626 -->

    <owl:NamedIndividual rdf:about="http://purl.obolibrary.org/obo/GAZ_00089626">
        <obo:RO_0001025 rdf:resource="http://purl.obolibrary.org/obo/GAZ_00056474"/>
        <obo:IAO_0000115>A paternoster lake in Hornopiren National Park.</obo:IAO_0000115>
        <oboInOwl:hasOBONamespace>GAZ</oboInOwl:hasOBONamespace>
        <oboInOwl:id>GAZ:00089626</oboInOwl:id>
        <rdfs:label>Lago Inexplorado</rdfs:label>
    </owl:NamedIndividual>
    


    <!-- http://purl.obolibrary.org/obo/GAZ_00089627 -->

    <owl:NamedIndividual rdf:about="http://purl.obolibrary.org/obo/GAZ_00089627">
        <obo:RO_0001025 rdf:resource="http://purl.obolibrary.org/obo/GAZ_00056474"/>
        <obo:IAO_0000115>A lake in Hornopiren National Park.</obo:IAO_0000115>
        <oboInOwl:hasOBONamespace>GAZ</oboInOwl:hasOBONamespace>
        <oboInOwl:id>GAZ:00089627</oboInOwl:id>
        <rdfs:label>Pinto Concha Lake</rdfs:label>
    </owl:NamedIndividual>
    


    <!-- http://purl.obolibrary.org/obo/GAZ_00089628 -->

    <owl:NamedIndividual rdf:about="http://purl.obolibrary.org/obo/GAZ_00089628">
        <obo:RO_0001025 rdf:resource="http://purl.obolibrary.org/obo/GAZ_00056474"/>
        <obo:IAO_0000115>A lake in Hornopiren National Park.</obo:IAO_0000115>
        <oboInOwl:hasOBONamespace>GAZ</oboInOwl:hasOBONamespace>
        <oboInOwl:id>GAZ:00089628</oboInOwl:id>
        <rdfs:label>Cabro Lake</rdfs:label>
    </owl:NamedIndividual>
    


    <!-- http://purl.obolibrary.org/obo/GAZ_00089634 -->

    <owl:NamedIndividual rdf:about="http://purl.obolibrary.org/obo/GAZ_00089634">
        <obo:RO_0001025 rdf:resource="http://purl.obolibrary.org/obo/GAZ_00056452"/>
        <obo:IAO_0000115>A lake located in the border of Los Lagos Region with Los Rios Region of Chile.</obo:IAO_0000115>
        <oboInOwl:hasOBONamespace>GAZ</oboInOwl:hasOBONamespace>
        <oboInOwl:id>GAZ:00089634</oboInOwl:id>
        <rdfs:label>Lago Puyehue</rdfs:label>
    </owl:NamedIndividual>
    


    <!-- http://purl.obolibrary.org/obo/GAZ_00089666 -->

    <owl:NamedIndividual rdf:about="http://purl.obolibrary.org/obo/GAZ_00089666">
        <obo:RO_0001025 rdf:resource="http://purl.obolibrary.org/obo/GAZ_00056260"/>
        <obo:IAO_0000115>A national park within the Cordillera Oriental mountain range in the Andes Mountains of Colombia.</obo:IAO_0000115>
        <oboInOwl:hasOBONamespace>GAZ</oboInOwl:hasOBONamespace>
        <oboInOwl:id>GAZ:00089666</oboInOwl:id>
        <rdfs:label>Parque Nacional El Cocuy</rdfs:label>
    </owl:NamedIndividual>
    


    <!-- http://purl.obolibrary.org/obo/GAZ_00089667 -->

    <owl:NamedIndividual rdf:about="http://purl.obolibrary.org/obo/GAZ_00089667">
        <rdf:type rdf:resource="http://purl.obolibrary.org/obo/ENVO_00000106"/>
        <obo:RO_0001025 rdf:resource="http://purl.obolibrary.org/obo/GAZ_00089666"/>
        <obo:IAO_0000115>A range within the Cordillera Oriental mountain range in the Andes Mountains of Colombia.</obo:IAO_0000115>
        <oboInOwl:hasOBONamespace>GAZ</oboInOwl:hasOBONamespace>
        <oboInOwl:id>GAZ:00089667</oboInOwl:id>
        <rdfs:label>Sierra Nevada del Cocuy</rdfs:label>
    </owl:NamedIndividual>
    


    <!-- http://purl.obolibrary.org/obo/GAZ_00089668 -->

    <owl:NamedIndividual rdf:about="http://purl.obolibrary.org/obo/GAZ_00089668">
        <obo:RO_0001025 rdf:resource="http://purl.obolibrary.org/obo/GAZ_22223509"/>
        <obo:IAO_0000115>A protected area, established in 1977, located in the Colombian Caribbean Region and the Guajira Peninsula and part of the department of La Guajira. The sanctuary is between the corregimiento of Camarones and the Tapias river, surrounded by marshes mainly the Manzanillo, Laguna Grande, Cienaga del Navio Quebrado and Tocoromanes marshes.</obo:IAO_0000115>
        <oboInOwl:hasOBONamespace>GAZ</oboInOwl:hasOBONamespace>
        <oboInOwl:id>GAZ:00089668</oboInOwl:id>
        <rdfs:label>Santuario de Fauna y Flora los Flamencos</rdfs:label>
    </owl:NamedIndividual>
    


    <!-- http://purl.obolibrary.org/obo/GAZ_00089671 -->

    <owl:NamedIndividual rdf:about="http://purl.obolibrary.org/obo/GAZ_00089671">
        <obo:IAO_0000115>A national park located in the central area of colombian Andes. In this park are located many places of interest, like Snow mountain of Ruiz, Snow Mountain of Tolima, Snow Mountain of St. Isabel, Swann snow mountain, Snow Mountain of Quindio, Otun Lake and Green Lake, among others. Established 1977.</obo:IAO_0000115>
        <oboInOwl:hasOBONamespace>GAZ</oboInOwl:hasOBONamespace>
        <oboInOwl:id>GAZ:00089671</oboInOwl:id>
        <rdfs:label>Parque Nacional de Los Nevados</rdfs:label>
    </owl:NamedIndividual>
    


    <!-- http://purl.obolibrary.org/obo/GAZ_00089675 -->

    <owl:NamedIndividual rdf:about="http://purl.obolibrary.org/obo/GAZ_00089675">
        <obo:RO_0001025 rdf:resource="http://purl.obolibrary.org/obo/GAZ_00056260"/>
        <obo:IAO_0000115>A mountain range that forms the southernmost spur of the Eastern Cordillera of the Andes, and is situated on the border of 4 distinct biogeographical regions: lowland Amazonia, the Eastern Cordillera, the Central Cordillera and the dryer Magdalena Valley.</obo:IAO_0000115>
        <oboInOwl:hasOBONamespace>GAZ</oboInOwl:hasOBONamespace>
        <oboInOwl:id>GAZ:00089675</oboInOwl:id>
        <rdfs:label>Serrania de los Churumbelos</rdfs:label>
    </owl:NamedIndividual>
    


    <!-- http://purl.obolibrary.org/obo/GAZ_00089676 -->

    <owl:NamedIndividual rdf:about="http://purl.obolibrary.org/obo/GAZ_00089676">
        <obo:RO_0001025 rdf:resource="http://purl.obolibrary.org/obo/GAZ_00089675"/>
        <obo:IAO_0000115>A national park that located in the Bota Caucana of southern Colombia. Established in 2007.</obo:IAO_0000115>
        <oboInOwl:hasOBONamespace>GAZ</oboInOwl:hasOBONamespace>
        <oboInOwl:id>GAZ:00089676</oboInOwl:id>
        <rdfs:label>Serrania de los Churumbelos National Park</rdfs:label>
    </owl:NamedIndividual>
    


    <!-- http://purl.obolibrary.org/obo/GAZ_00089680 -->

    <owl:NamedIndividual rdf:about="http://purl.obolibrary.org/obo/GAZ_00089680">
        <obo:RO_0001025 rdf:resource="http://purl.obolibrary.org/obo/GAZ_22223509"/>
        <obo:IAO_0000115>A protected area located in north Colombia, in the La Guajira Department.</obo:IAO_0000115>
        <oboInOwl:hasOBONamespace>GAZ</oboInOwl:hasOBONamespace>
        <oboInOwl:id>GAZ:00089680</oboInOwl:id>
        <rdfs:label>Bahia Portete Fauna and Flora Sanctuary</rdfs:label>
    </owl:NamedIndividual>
    


    <!-- http://purl.obolibrary.org/obo/GAZ_00089687 -->

    <owl:NamedIndividual rdf:about="http://purl.obolibrary.org/obo/GAZ_00089687">
        <obo:RO_0001025 rdf:resource="http://purl.obolibrary.org/obo/GAZ_00056254"/>
        <obo:IAO_0000115>A protected area located near the Purace National Park in the Department of Huila, within the municipalities of Saladoblanco, Oporapa, Tarqui, La Plata, El Pital and La Argentina.</obo:IAO_0000115>
        <oboInOwl:hasOBONamespace>GAZ</oboInOwl:hasOBONamespace>
        <oboInOwl:id>GAZ:00089687</oboInOwl:id>
        <rdfs:label>Serrania de Minas Fauna and Flora Sanctuary</rdfs:label>
    </owl:NamedIndividual>
    


    <!-- http://purl.obolibrary.org/obo/GAZ_00089691 -->

    <owl:NamedIndividual rdf:about="http://purl.obolibrary.org/obo/GAZ_00089691">
        <obo:RO_0001025 rdf:resource="http://purl.obolibrary.org/obo/GAZ_00056260"/>
        <obo:IAO_0000115>A national park.</obo:IAO_0000115>
        <oboInOwl:hasOBONamespace>GAZ</oboInOwl:hasOBONamespace>
        <oboInOwl:id>GAZ:00089691</oboInOwl:id>
        <rdfs:label>Parque Nacional Chingaza</rdfs:label>
    </owl:NamedIndividual>
    


    <!-- http://purl.obolibrary.org/obo/GAZ_00089694 -->

    <owl:NamedIndividual rdf:about="http://purl.obolibrary.org/obo/GAZ_00089694">
        <obo:RO_0001025 rdf:resource="http://purl.obolibrary.org/obo/GAZ_00056260"/>
        <obo:IAO_0000115>A national park.</obo:IAO_0000115>
        <oboInOwl:hasOBONamespace>GAZ</oboInOwl:hasOBONamespace>
        <oboInOwl:id>GAZ:00089694</oboInOwl:id>
        <rdfs:label>Parque Nacional Cordillera de los Picachos</rdfs:label>
    </owl:NamedIndividual>
    


    <!-- http://purl.obolibrary.org/obo/GAZ_00089697 -->

    <owl:NamedIndividual rdf:about="http://purl.obolibrary.org/obo/GAZ_00089697">
        <obo:RO_0001025 rdf:resource="http://purl.obolibrary.org/obo/GAZ_00056254"/>
        <obo:IAO_0000115>A national park.</obo:IAO_0000115>
        <oboInOwl:hasOBONamespace>GAZ</oboInOwl:hasOBONamespace>
        <oboInOwl:id>GAZ:00089697</oboInOwl:id>
        <rdfs:label>Parque Nacional Las Hermosas</rdfs:label>
    </owl:NamedIndividual>
    


    <!-- http://purl.obolibrary.org/obo/GAZ_00089698 -->

    <owl:NamedIndividual rdf:about="http://purl.obolibrary.org/obo/GAZ_00089698">
        <obo:RO_0001025 rdf:resource="http://purl.obolibrary.org/obo/GAZ_00056247"/>
        <obo:IAO_0000115>A national park.</obo:IAO_0000115>
        <oboInOwl:hasOBONamespace>GAZ</oboInOwl:hasOBONamespace>
        <oboInOwl:id>GAZ:00089698</oboInOwl:id>
        <rdfs:label>Parque Nacional de Las Orquideas</rdfs:label>
    </owl:NamedIndividual>
    


    <!-- http://purl.obolibrary.org/obo/GAZ_00089699 -->

    <owl:NamedIndividual rdf:about="http://purl.obolibrary.org/obo/GAZ_00089699">
        <obo:RO_0001025 rdf:resource="http://purl.obolibrary.org/obo/GAZ_00056254"/>
        <obo:IAO_0000115>A national park.</obo:IAO_0000115>
        <oboInOwl:hasOBONamespace>GAZ</oboInOwl:hasOBONamespace>
        <oboInOwl:id>GAZ:00089699</oboInOwl:id>
        <rdfs:label>Parque Nacional del Nevado del Huila</rdfs:label>
    </owl:NamedIndividual>
    


    <!-- http://purl.obolibrary.org/obo/GAZ_00089700 -->

    <owl:NamedIndividual rdf:about="http://purl.obolibrary.org/obo/GAZ_00089700">
        <obo:RO_0001025 rdf:resource="http://purl.obolibrary.org/obo/GAZ_00056247"/>
        <obo:IAO_0000115>A national park.</obo:IAO_0000115>
        <oboInOwl:hasOBONamespace>GAZ</oboInOwl:hasOBONamespace>
        <oboInOwl:id>GAZ:00089700</oboInOwl:id>
        <rdfs:label>Parque Nacional Paramillo</rdfs:label>
    </owl:NamedIndividual>
    


    <!-- http://purl.obolibrary.org/obo/GAZ_00089701 -->

    <owl:NamedIndividual rdf:about="http://purl.obolibrary.org/obo/GAZ_00089701">
        <obo:RO_0001025 rdf:resource="http://purl.obolibrary.org/obo/GAZ_00056260"/>
        <obo:IAO_0000115>A national park.</obo:IAO_0000115>
        <oboInOwl:hasOBONamespace>GAZ</oboInOwl:hasOBONamespace>
        <oboInOwl:id>GAZ:00089701</oboInOwl:id>
        <rdfs:label>Parque Nacional Pisba</rdfs:label>
    </owl:NamedIndividual>
    


    <!-- http://purl.obolibrary.org/obo/GAZ_00089702 -->

    <owl:NamedIndividual rdf:about="http://purl.obolibrary.org/obo/GAZ_00089702">
        <obo:RO_0001025 rdf:resource="http://purl.obolibrary.org/obo/GAZ_00056254"/>
        <obo:IAO_0000115>A national park. Established 1961; enlarged 1977.</obo:IAO_0000115>
        <oboInOwl:hasOBONamespace>GAZ</oboInOwl:hasOBONamespace>
        <oboInOwl:id>GAZ:00089702</oboInOwl:id>
        <rdfs:label>Parque Nacional Purace</rdfs:label>
    </owl:NamedIndividual>
    


    <!-- http://purl.obolibrary.org/obo/GAZ_00089706 -->

    <owl:NamedIndividual rdf:about="http://purl.obolibrary.org/obo/GAZ_00089706">
        <obo:RO_0001025 rdf:resource="http://purl.obolibrary.org/obo/GAZ_00056247"/>
        <obo:IAO_0000115>A national park.</obo:IAO_0000115>
        <oboInOwl:hasOBONamespace>GAZ</oboInOwl:hasOBONamespace>
        <oboInOwl:id>GAZ:00089706</oboInOwl:id>
        <rdfs:label>Parque Nacional Tatama</rdfs:label>
    </owl:NamedIndividual>
    


    <!-- http://purl.obolibrary.org/obo/GAZ_00090268 -->

    <owl:NamedIndividual rdf:about="http://purl.obolibrary.org/obo/GAZ_00090268">
        <obo:RO_0001025 rdf:resource="http://purl.obolibrary.org/obo/GAZ_00056605"/>
        <obo:IAO_0000115>A national park in the Cordillera Blanca, a range of the Andes, in Ancash of central Peru. A World Heritage Site. Established 1975-07-01.</obo:IAO_0000115>
        <oboInOwl:hasOBONamespace>GAZ</oboInOwl:hasOBONamespace>
        <oboInOwl:id>GAZ:00090268</oboInOwl:id>
        <rdfs:label>Parque Nacional Huascaran</rdfs:label>
    </owl:NamedIndividual>
    


    <!-- http://purl.obolibrary.org/obo/GAZ_00103640 -->

    <owl:NamedIndividual rdf:about="http://purl.obolibrary.org/obo/GAZ_00103640">
        <obo:RO_0001025 rdf:resource="http://purl.obolibrary.org/obo/GAZ_22223491"/>
        <obo:IAO_0000115>El parque comprende gran parte de las costas araguenas y de la zona montanosa del Estado Carabobo, ademas colinda con el Parque Nacional San Esteban.</obo:IAO_0000115>
        <oboInOwl:hasOBONamespace>GAZ</oboInOwl:hasOBONamespace>
        <oboInOwl:id>GAZ:00103640</oboInOwl:id>
        <rdfs:label>Parque Nacional Henri Pittier</rdfs:label>
    </owl:NamedIndividual>
    


    <!-- http://purl.obolibrary.org/obo/GAZ_00103641 -->

    <owl:NamedIndividual rdf:about="http://purl.obolibrary.org/obo/GAZ_00103641">
        <obo:RO_0001025 rdf:resource="http://purl.obolibrary.org/obo/GAZ_00103640"/>
        <oboInOwl:hasOBONamespace>GAZ</oboInOwl:hasOBONamespace>
        <oboInOwl:id>GAZ:00103641</oboInOwl:id>
        <rdfs:label>Estacion Biologica Alberto Fernandez Yepez</rdfs:label>
    </owl:NamedIndividual>
    


    <!-- http://purl.obolibrary.org/obo/GAZ_00103674 -->

    <owl:NamedIndividual rdf:about="http://purl.obolibrary.org/obo/GAZ_00103674">
        <obo:RO_0001025 rdf:resource="http://purl.obolibrary.org/obo/GAZ_00056705"/>
        <obo:IAO_0000115>A caldera in Catamarca Province, Argentina, considered to be the best exposed large caldera in the world. It was formed 2.2 million years ago when 1,050 km3 of material was erupted, producing ignimbrite deposits stretching up to 100 km away. The caldera was originally the site of a large lake, but resurgence of the eastern caldera floor has confined the salty Laguna Diamante to the caldera&apos;s western edge.</obo:IAO_0000115>
        <oboInOwl:hasOBONamespace>GAZ</oboInOwl:hasOBONamespace>
        <oboInOwl:id>GAZ:00103674</oboInOwl:id>
        <rdfs:label>Cerro Galan Caldera</rdfs:label>
    </owl:NamedIndividual>
    


    <!-- http://purl.obolibrary.org/obo/GAZ_00103675 -->

    <owl:NamedIndividual rdf:about="http://purl.obolibrary.org/obo/GAZ_00103675">
        <obo:RO_0001025 rdf:resource="http://purl.obolibrary.org/obo/GAZ_00103674"/>
        <obo:IAO_0000115>A saline caldera lake.</obo:IAO_0000115>
        <oboInOwl:hasOBONamespace>GAZ</oboInOwl:hasOBONamespace>
        <oboInOwl:id>GAZ:00103675</oboInOwl:id>
        <rdfs:label>Laguna Diamante</rdfs:label>
    </owl:NamedIndividual>
    


    <!-- http://purl.obolibrary.org/obo/GAZ_00120032 -->

    <owl:NamedIndividual rdf:about="http://purl.obolibrary.org/obo/GAZ_00120032">
        <obo:IAO_0000115>Un lago tectonico con una profundidad de 3,5 metros que rodea al salar homonimo, y al cono volcanico de Villa Pucarani con una altura de 4.910 msnm. Este lago esta situado a una altura de 3.657 msnm, en el Departamento de Oruro, Bolivia. El principal rio que desemboca en el lago es el rio Lauca, proveniente de Chile.</obo:IAO_0000115>
        <oboInOwl:hasOBONamespace>GAZ</oboInOwl:hasOBONamespace>
        <oboInOwl:id>GAZ:00120032</oboInOwl:id>
        <rdfs:label>Lago Coipasa</rdfs:label>
    </owl:NamedIndividual>
    


    <!-- http://purl.obolibrary.org/obo/GAZ_00120476 -->

    <owl:NamedIndividual rdf:about="http://purl.obolibrary.org/obo/GAZ_00120476">
        <obo:IAO_0000115>A saline lake.</obo:IAO_0000115>
        <oboInOwl:hasOBONamespace>GAZ</oboInOwl:hasOBONamespace>
        <oboInOwl:id>GAZ:00120476</oboInOwl:id>
        <rdfs:label>Laguna Celeste</rdfs:label>
    </owl:NamedIndividual>
    


    <!-- http://purl.obolibrary.org/obo/GAZ_00120477 -->

    <owl:NamedIndividual rdf:about="http://purl.obolibrary.org/obo/GAZ_00120477">
        <obo:IAO_0000115>A protected area.</obo:IAO_0000115>
        <oboInOwl:hasOBONamespace>GAZ</oboInOwl:hasOBONamespace>
        <oboInOwl:id>GAZ:00120477</oboInOwl:id>
        <rdfs:label>Reserva Nacional de Fauna Andina Eduardo Abaroa</rdfs:label>
    </owl:NamedIndividual>
    


    <!-- http://purl.obolibrary.org/obo/GAZ_00120478 -->

    <owl:NamedIndividual rdf:about="http://purl.obolibrary.org/obo/GAZ_00120478">
        <obo:RO_0001025 rdf:resource="http://purl.obolibrary.org/obo/GAZ_00120477"/>
        <obo:IAO_0000115>A freshwater lake.</obo:IAO_0000115>
        <oboInOwl:hasOBONamespace>GAZ</oboInOwl:hasOBONamespace>
        <oboInOwl:id>GAZ:00120478</oboInOwl:id>
        <rdfs:label>Laguna Kalina</rdfs:label>
    </owl:NamedIndividual>
    


    <!-- http://purl.obolibrary.org/obo/GAZ_00120479 -->

    <owl:NamedIndividual rdf:about="http://purl.obolibrary.org/obo/GAZ_00120479">
        <obo:RO_0001025 rdf:resource="http://purl.obolibrary.org/obo/GAZ_00120477"/>
        <obo:IAO_0000115>A freshwater lake.</obo:IAO_0000115>
        <oboInOwl:hasOBONamespace>GAZ</oboInOwl:hasOBONamespace>
        <oboInOwl:id>GAZ:00120479</oboInOwl:id>
        <rdfs:label>Laguna Coruto</rdfs:label>
    </owl:NamedIndividual>
    


    <!-- http://purl.obolibrary.org/obo/GAZ_00120627 -->

    <owl:NamedIndividual rdf:about="http://purl.obolibrary.org/obo/GAZ_00120627">
        <obo:RO_0001025 rdf:resource="http://purl.obolibrary.org/obo/GAZ_00120477"/>
        <obo:IAO_0000115>Una laguna alto-andina situada dentro de la Reserva Nacional de Fauna Andina Eduardo Abaroa, en el departamento de Potosi, Bolivia.</obo:IAO_0000115>
        <oboInOwl:hasOBONamespace>GAZ</oboInOwl:hasOBONamespace>
        <oboInOwl:id>GAZ:00120627</oboInOwl:id>
        <rdfs:label>Laguna Blanca</rdfs:label>
    </owl:NamedIndividual>
    


    <!-- http://purl.obolibrary.org/obo/GAZ_00120628 -->

    <owl:NamedIndividual rdf:about="http://purl.obolibrary.org/obo/GAZ_00120628">
        <obo:RO_0001025 rdf:resource="http://purl.obolibrary.org/obo/GAZ_00120477"/>
        <obo:IAO_0000115>Un area de aproximadamente 2 km2 de extension, ubicada en el departamento de Potosi, Bolivia, al sur de la Laguna Colorada en el camino hacia el Salar de Chalviri, a una altura de 4.850 msnm. Esta area se caracteriza por tener intensa actividad volcanica y fomarolica (Geiseres), en los crateres ubicados en la region se puede observar lava hirviendo intensamente; adicionalmente, las fumarolas (geiser) emiten vapores mixtos de agua y vapor caliente que alcanzan alturas de 10 a 50 metros, producto de la presion con los que son emitidos; estos fenomenos permiten apreciar un paisaje que remonta a las epocas de la formacion de la tierra.</obo:IAO_0000115>
        <oboInOwl:hasOBONamespace>GAZ</oboInOwl:hasOBONamespace>
        <oboInOwl:id>GAZ:00120628</oboInOwl:id>
        <rdfs:label>Sol de Manana</rdfs:label>
    </owl:NamedIndividual>
    


    <!-- http://purl.obolibrary.org/obo/GAZ_00120669 -->

    <owl:NamedIndividual rdf:about="http://purl.obolibrary.org/obo/GAZ_00120669">
        <obo:RO_0001025 rdf:resource="http://purl.obolibrary.org/obo/GAZ_00120477"/>
        <obo:IAO_0000115>Una laguna de agua dulce ubicada al sur del departamento boliviano de Potosi.</obo:IAO_0000115>
        <oboInOwl:hasOBONamespace>GAZ</oboInOwl:hasOBONamespace>
        <oboInOwl:id>GAZ:00120669</oboInOwl:id>
        <rdfs:label>Laguna Chojllas</rdfs:label>
    </owl:NamedIndividual>
    


    <!-- http://purl.obolibrary.org/obo/GAZ_00120670 -->

    <owl:NamedIndividual rdf:about="http://purl.obolibrary.org/obo/GAZ_00120670">
        <obo:IAO_0000115>Una cadena montanosa de los andes, nace en la frontera de Peru-Bolivia, al norte de lago Titicaca, especificamente en el Nevado Chaupi Orco y los tres Palomanis, adentrandose en territorio boliviano en el noreste del departamento de La Paz, terminando en la altiplanicie de Guarayos.</obo:IAO_0000115>
        <oboInOwl:hasOBONamespace>GAZ</oboInOwl:hasOBONamespace>
        <oboInOwl:id>GAZ:00120670</oboInOwl:id>
        <rdfs:label>Cordillera de Apolobamba</rdfs:label>
    </owl:NamedIndividual>
    


    <!-- http://purl.obolibrary.org/obo/GAZ_00120671 -->

    <owl:NamedIndividual rdf:about="http://purl.obolibrary.org/obo/GAZ_00120671">
        <obo:RO_0001025 rdf:resource="http://purl.obolibrary.org/obo/GAZ_00120670"/>
        <obo:IAO_0000115>Un cuerpo de agua producto de deshielos de glaciares proximos a el, se encuentra entre los departamentos de La Paz, Bolivia y Puno en Peru, formando frontera natural entre los dos paises, se encuentra dentro del Area Natural de Manejo Integrado Apolobamba en la cordillera de Apolobamba.</obo:IAO_0000115>
        <oboInOwl:hasOBONamespace>GAZ</oboInOwl:hasOBONamespace>
        <oboInOwl:id>GAZ:00120671</oboInOwl:id>
        <rdfs:label>Laguna Suches</rdfs:label>
    </owl:NamedIndividual>
    


    <!-- http://purl.obolibrary.org/obo/GAZ_00120672 -->

    <owl:NamedIndividual rdf:about="http://purl.obolibrary.org/obo/GAZ_00120672">
        <obo:RO_0001025 rdf:resource="http://purl.obolibrary.org/obo/GAZ_00120670"/>
        <obo:IAO_0000115>Una laguna altoandina localizada en el departamentos de La Paz, Bolivia. Y se encuentra en la Cordillera de Apolobamba como muchas otras lagunas del entorno presenta una forma alargada y estrecha.</obo:IAO_0000115>
        <oboInOwl:hasOBONamespace>GAZ</oboInOwl:hasOBONamespace>
        <oboInOwl:id>GAZ:00120672</oboInOwl:id>
        <rdfs:label>Laguna Cololo</rdfs:label>
    </owl:NamedIndividual>
    


    <!-- http://purl.obolibrary.org/obo/GAZ_00120695 -->

    <owl:NamedIndividual rdf:about="http://purl.obolibrary.org/obo/GAZ_00120695">
        <obo:RO_0001025 rdf:resource="http://purl.obolibrary.org/obo/GAZ_00120477"/>
        <obo:IAO_0000115>Una laguna salina altoandina, ubicada al sur del departamento de Potosi, al sur de Bolivia dentro de la Reserva Nacional de Fauna Andina Eduardo Abaroa.</obo:IAO_0000115>
        <oboInOwl:hasOBONamespace>GAZ</oboInOwl:hasOBONamespace>
        <oboInOwl:id>GAZ:00120695</oboInOwl:id>
        <rdfs:label>Laguna Guayaques</rdfs:label>
    </owl:NamedIndividual>
    


    <!-- http://purl.obolibrary.org/obo/GAZ_00120707 -->

    <owl:NamedIndividual rdf:about="http://purl.obolibrary.org/obo/GAZ_00120707">
        <obo:RO_0001025 rdf:resource="http://purl.obolibrary.org/obo/GAZ_00120477"/>
        <obo:IAO_0000115>Un desierto boliviano ubicado al sur del departamento de Potosi dentro de la Reserva Nacional de Fauna Andina Eduardo.</obo:IAO_0000115>
        <oboInOwl:hasOBONamespace>GAZ</oboInOwl:hasOBONamespace>
        <oboInOwl:id>GAZ:00120707</oboInOwl:id>
        <rdfs:label>Desierto Salvador Dali</rdfs:label>
    </owl:NamedIndividual>
    


    <!-- http://purl.obolibrary.org/obo/GAZ_00120718 -->

    <owl:NamedIndividual rdf:about="http://purl.obolibrary.org/obo/GAZ_00120718">
        <obo:RO_0001025 rdf:resource="http://purl.obolibrary.org/obo/GAZ_00138618"/>
        <obo:IAO_0000115>A group of saline lakes. Fed by underground sources and with a high sulfur content.</obo:IAO_0000115>
        <oboInOwl:hasOBONamespace>GAZ</oboInOwl:hasOBONamespace>
        <oboInOwl:id>GAZ:00120718</oboInOwl:id>
        <rdfs:label>Lagunas Pastos Grandes</rdfs:label>
    </owl:NamedIndividual>
    


    <!-- http://purl.obolibrary.org/obo/GAZ_00120725 -->

    <owl:NamedIndividual rdf:about="http://purl.obolibrary.org/obo/GAZ_00120725">
        <obo:RO_0001025 rdf:resource="http://purl.obolibrary.org/obo/GAZ_00056425"/>
        <obo:IAO_0000115>Una pequena laguna boliviana situada a los pies del volcan Sajama el punto mas alto del pais, en el departamento de Oruro.</obo:IAO_0000115>
        <oboInOwl:hasOBONamespace>GAZ</oboInOwl:hasOBONamespace>
        <oboInOwl:id>GAZ:00120725</oboInOwl:id>
        <rdfs:label>Laguna Sajama</rdfs:label>
    </owl:NamedIndividual>
    


    <!-- http://purl.obolibrary.org/obo/GAZ_00120745 -->

    <owl:NamedIndividual rdf:about="http://purl.obolibrary.org/obo/GAZ_00120745">
        <obo:RO_0001025 rdf:resource="http://purl.obolibrary.org/obo/GAZ_00120746"/>
        <obo:IAO_0000115>Una isla fluvial boliviana situada al este del departamento del Beni en las coordenadas, en la frontera con Brasil, la isla se encuentra completamente rodeada por el rio Itenez.</obo:IAO_0000115>
        <oboInOwl:hasOBONamespace>GAZ</oboInOwl:hasOBONamespace>
        <oboInOwl:id>GAZ:00120745</oboInOwl:id>
        <rdfs:label>Isla Cumprida</rdfs:label>
    </owl:NamedIndividual>
    


    <!-- http://purl.obolibrary.org/obo/GAZ_00120746 -->

    <owl:NamedIndividual rdf:about="http://purl.obolibrary.org/obo/GAZ_00120746">
        <obo:IAO_0000115>Un rio boliviano - brasileno, perteneciente a la cuenca del amazonas, nace en Brasil donde recorre en direccion nor-oeste unos 560 kilometros en territorio brasileno hasta uno de sus afluente llamado rio Verde donde pasa a formar una frontera natural entre los dos paises de 970 kilometros hasta su desembocadura en el rio Mamore.</obo:IAO_0000115>
        <oboInOwl:hasOBONamespace>GAZ</oboInOwl:hasOBONamespace>
        <oboInOwl:id>GAZ:00120746</oboInOwl:id>
        <rdfs:label>Rio Itenez</rdfs:label>
    </owl:NamedIndividual>
    


    <!-- http://purl.obolibrary.org/obo/GAZ_00120747 -->

    <owl:NamedIndividual rdf:about="http://purl.obolibrary.org/obo/GAZ_00120747">
        <obo:IAO_0000115>Un rio amazonico boliviano-brasilero, aunque la mayor parte de su recorrido lo hace en territorio boliviano siendo este el mas importante del pais, pertenece a la cuenca del Amazonas, nace de las confluencias de los rios Chapare y Mamorecillo en las coordenadas entre los departamentos de Santa Cruz y Cochabamba, a 24 kilometros al sur de la desembocadura de uno de sus grandes afluentes el rio Grande, el rio discurre en direccion norte en todo su recorrido, aunque el algunas zonas discurre en direccion noroeste y noreste.</obo:IAO_0000115>
        <oboInOwl:hasOBONamespace>GAZ</oboInOwl:hasOBONamespace>
        <oboInOwl:id>GAZ:00120747</oboInOwl:id>
        <rdfs:label>Rio Mamore</rdfs:label>
    </owl:NamedIndividual>
    


    <!-- http://purl.obolibrary.org/obo/GAZ_00120748 -->

    <owl:NamedIndividual rdf:about="http://purl.obolibrary.org/obo/GAZ_00120748">
        <obo:RO_0001025 rdf:resource="http://purl.obolibrary.org/obo/GAZ_00120747"/>
        <obo:IAO_0000115>Una isla fluvial amazonica ubicada sobre el rio Mamore. La soberania sobre la isla esta en disputa pasiva entre Brasil y Bolivia. Para Bolivia la isla forma parte del Departamento del Beni y para Brasil es parte del Municipio de Guajara-Mirim en el estado de Rondonia.</obo:IAO_0000115>
        <oboInOwl:hasOBONamespace>GAZ</oboInOwl:hasOBONamespace>
        <oboInOwl:id>GAZ:00120748</oboInOwl:id>
        <rdfs:label>Isla Suarez</rdfs:label>
    </owl:NamedIndividual>
    


    <!-- http://purl.obolibrary.org/obo/GAZ_00121007 -->

    <owl:NamedIndividual rdf:about="http://purl.obolibrary.org/obo/GAZ_00121007">
        <obo:RO_0001025 rdf:resource="http://purl.obolibrary.org/obo/GAZ_00056694"/>
        <obo:IAO_0000115>A freshwater lake. Un lago ubicado en la Provincia de Parinacota, Region de Arica y Parinacota, Chile.</obo:IAO_0000115>
        <oboInOwl:hasOBONamespace>GAZ</oboInOwl:hasOBONamespace>
        <oboInOwl:id>GAZ:00121007</oboInOwl:id>
        <rdfs:label>Lago Chungara</rdfs:label>
    </owl:NamedIndividual>
    


    <!-- http://purl.obolibrary.org/obo/GAZ_00121008 -->

    <owl:NamedIndividual rdf:about="http://purl.obolibrary.org/obo/GAZ_00121008">
        <obo:RO_0001025 rdf:resource="http://purl.obolibrary.org/obo/GAZ_00056408"/>
        <obo:IAO_0000115>A crater lake.</obo:IAO_0000115>
        <oboInOwl:hasOBONamespace>GAZ</oboInOwl:hasOBONamespace>
        <oboInOwl:id>GAZ:00121008</oboInOwl:id>
        <rdfs:label>Lago Licancabur</rdfs:label>
    </owl:NamedIndividual>
    


    <!-- http://purl.obolibrary.org/obo/GAZ_00121645 -->

    <owl:NamedIndividual rdf:about="http://purl.obolibrary.org/obo/GAZ_00121645">
        <obo:RO_0001025 rdf:resource="http://purl.obolibrary.org/obo/GAZ_00056605"/>
        <obo:IAO_0000115>A glacier lake.</obo:IAO_0000115>
        <oboInOwl:hasOBONamespace>GAZ</oboInOwl:hasOBONamespace>
        <oboInOwl:id>GAZ:00121645</oboInOwl:id>
        <rdfs:label>Laguna Santa Cruz Chica</rdfs:label>
    </owl:NamedIndividual>
    


    <!-- http://purl.obolibrary.org/obo/GAZ_00121646 -->

    <owl:NamedIndividual rdf:about="http://purl.obolibrary.org/obo/GAZ_00121646">
        <obo:RO_0001025 rdf:resource="http://purl.obolibrary.org/obo/GAZ_00056605"/>
        <obo:IAO_0000115>A glacier lake. It is located just north of Huandoy mountain, in Caraz.</obo:IAO_0000115>
        <oboInOwl:hasOBONamespace>GAZ</oboInOwl:hasOBONamespace>
        <oboInOwl:id>GAZ:00121646</oboInOwl:id>
        <rdfs:label>Laguna de Paron</rdfs:label>
    </owl:NamedIndividual>
    


    <!-- http://purl.obolibrary.org/obo/GAZ_00121647 -->

    <owl:NamedIndividual rdf:about="http://purl.obolibrary.org/obo/GAZ_00121647">
        <obo:RO_0001025 rdf:resource="http://purl.obolibrary.org/obo/GAZ_00090268"/>
        <obo:IAO_0000115>Un estrecho valle glaciar, flanqueadas por los montes nevados Huascaran, Huandoy, Pishqo, Shapraraju, Yanapaccha y Chopicalqui (Cordillera Blanca), el sendero de Maria Josefa y la Quebrada Demanda, formando parte del Parque Nacional Huascaran y la Reserva de la biosfera del Huascaran.</obo:IAO_0000115>
        <oboInOwl:hasOBONamespace>GAZ</oboInOwl:hasOBONamespace>
        <oboInOwl:id>GAZ:00121647</oboInOwl:id>
        <rdfs:label>Llanganuco Valley</rdfs:label>
    </owl:NamedIndividual>
    


    <!-- http://purl.obolibrary.org/obo/GAZ_00121648 -->

    <owl:NamedIndividual rdf:about="http://purl.obolibrary.org/obo/GAZ_00121648">
        <obo:RO_0001025 rdf:resource="http://purl.obolibrary.org/obo/GAZ_00121647"/>
        <obo:IAO_0000115>A glacier lake.</obo:IAO_0000115>
        <oboInOwl:hasOBONamespace>GAZ</oboInOwl:hasOBONamespace>
        <oboInOwl:id>GAZ:00121648</oboInOwl:id>
        <rdfs:label>Laguna Orconcocha</rdfs:label>
    </owl:NamedIndividual>
    


    <!-- http://purl.obolibrary.org/obo/GAZ_00121649 -->

    <owl:NamedIndividual rdf:about="http://purl.obolibrary.org/obo/GAZ_00121649">
        <obo:RO_0001025 rdf:resource="http://purl.obolibrary.org/obo/GAZ_00121647"/>
        <obo:IAO_0000115>A glacier lake.</obo:IAO_0000115>
        <oboInOwl:hasOBONamespace>GAZ</oboInOwl:hasOBONamespace>
        <oboInOwl:id>GAZ:00121649</oboInOwl:id>
        <rdfs:label>Laguna Chinancocha</rdfs:label>
    </owl:NamedIndividual>
    


    <!-- http://purl.obolibrary.org/obo/GAZ_00121650 -->

    <owl:NamedIndividual rdf:about="http://purl.obolibrary.org/obo/GAZ_00121650">
        <obo:RO_0001025 rdf:resource="http://purl.obolibrary.org/obo/GAZ_00056605"/>
        <obo:IAO_0000115>A glacier lake.</obo:IAO_0000115>
        <oboInOwl:hasOBONamespace>GAZ</oboInOwl:hasOBONamespace>
        <oboInOwl:id>GAZ:00121650</oboInOwl:id>
        <rdfs:label>Laguna Santa Cruz Grande</rdfs:label>
    </owl:NamedIndividual>
    


    <!-- http://purl.obolibrary.org/obo/GAZ_00130253 -->

    <owl:NamedIndividual rdf:about="http://purl.obolibrary.org/obo/GAZ_00130253">
        <obo:RO_0001025 rdf:resource="http://purl.obolibrary.org/obo/GAZ_00121647"/>
        <obo:IAO_0000115>A lake.</obo:IAO_0000115>
        <oboInOwl:hasOBONamespace>GAZ</oboInOwl:hasOBONamespace>
        <oboInOwl:id>GAZ:00130253</oboInOwl:id>
        <rdfs:label>Laguna Llanganuco</rdfs:label>
    </owl:NamedIndividual>
    


    <!-- http://purl.obolibrary.org/obo/GAZ_00136448 -->

    <owl:NamedIndividual rdf:about="http://purl.obolibrary.org/obo/GAZ_00136448">
        <obo:IAO_0000115>A volcanic arc in northwestern South America. It is one of the four volcanic zones of the Andes. The North Volcanic Zone extends from Colombia to Ecuador. The volcanic arc has formed due to subduction of the Nazca Plate under western South America. Between 6degN and 3degS.</obo:IAO_0000115>
        <oboInOwl:hasOBONamespace>GAZ</oboInOwl:hasOBONamespace>
        <oboInOwl:id>GAZ:00136448</oboInOwl:id>
        <rdfs:label>North Volcanic Zone</rdfs:label>
    </owl:NamedIndividual>
    


    <!-- http://purl.obolibrary.org/obo/GAZ_00136449 -->

    <owl:NamedIndividual rdf:about="http://purl.obolibrary.org/obo/GAZ_00136449">
        <obo:IAO_0000115>A volcanic arc in western South America. It is one of the four volcanic zones of the Andes. The Central Volcanic Zone extends from Peru to Chile and forms the western boundary of the Altiplano plateau. The volcanic arc has formed due to subduction of the Nazca Plate under western South America along the Peru-Chile Trench. Between 15degS and 27degS.</obo:IAO_0000115>
        <oboInOwl:hasOBONamespace>GAZ</oboInOwl:hasOBONamespace>
        <oboInOwl:id>GAZ:00136449</oboInOwl:id>
        <rdfs:label>Central Volcanic Zone</rdfs:label>
    </owl:NamedIndividual>
    


    <!-- http://purl.obolibrary.org/obo/GAZ_00136450 -->

    <owl:NamedIndividual rdf:about="http://purl.obolibrary.org/obo/GAZ_00136450">
        <obo:RO_0001025 rdf:resource="http://purl.obolibrary.org/obo/GAZ_00136449"/>
        <obo:IAO_0000115>A volcano in Peru.</obo:IAO_0000115>
        <oboInOwl:hasOBONamespace>GAZ</oboInOwl:hasOBONamespace>
        <oboInOwl:id>GAZ:00136450</oboInOwl:id>
        <rdfs:label>Volcan Chupiquina</rdfs:label>
    </owl:NamedIndividual>
    


    <!-- http://purl.obolibrary.org/obo/GAZ_00136451 -->

    <owl:NamedIndividual rdf:about="http://purl.obolibrary.org/obo/GAZ_00136451">
        <obo:RO_0001025 rdf:resource="http://purl.obolibrary.org/obo/GAZ_00136449"/>
        <obo:IAO_0000115>A volcano in Peru.</obo:IAO_0000115>
        <oboInOwl:hasOBONamespace>GAZ</oboInOwl:hasOBONamespace>
        <oboInOwl:id>GAZ:00136451</oboInOwl:id>
        <rdfs:label>Volcan Tacune Ubinas</rdfs:label>
    </owl:NamedIndividual>
    


    <!-- http://purl.obolibrary.org/obo/GAZ_00136452 -->

    <owl:NamedIndividual rdf:about="http://purl.obolibrary.org/obo/GAZ_00136452">
        <obo:RO_0001025 rdf:resource="http://purl.obolibrary.org/obo/GAZ_00136449"/>
        <obo:IAO_0000115>A volcano in Peru.</obo:IAO_0000115>
        <oboInOwl:hasOBONamespace>GAZ</oboInOwl:hasOBONamespace>
        <oboInOwl:id>GAZ:00136452</oboInOwl:id>
        <rdfs:label>Volcan Pichu Pichu</rdfs:label>
    </owl:NamedIndividual>
    


    <!-- http://purl.obolibrary.org/obo/GAZ_00136453 -->

    <owl:NamedIndividual rdf:about="http://purl.obolibrary.org/obo/GAZ_00136453">
        <obo:IAO_0000115>A volcanic arc in southwestern South America. It is one of the four volcanic zones of the Andes. The SVZ extends roughly from Central Chile&apos;s Andes at the latitude of Santiago to Mount Hudson in Aysen Region, a distance of well over 1,400 km. The arc has formed due to subduction of Nazca Plate under the South American Plate along the Peru-Chile Trench. The northern boundary of the SVZ is marked by the flat-slab subduction of the Juan Fernandez Ridge, which has produced a &quot;volcanic gap&quot; in the Norte Chico region. The southern end of the SVZ is marked by the Chile Triple Junction where the Chile Rise subducts under southamerica at Taitao Peninsula. Between 33degS and 46degS.</obo:IAO_0000115>
        <oboInOwl:hasOBONamespace>GAZ</oboInOwl:hasOBONamespace>
        <oboInOwl:id>GAZ:00136453</oboInOwl:id>
        <rdfs:label>South Volcanic Zone</rdfs:label>
    </owl:NamedIndividual>
    


    <!-- http://purl.obolibrary.org/obo/GAZ_00136454 -->

    <owl:NamedIndividual rdf:about="http://purl.obolibrary.org/obo/GAZ_00136454">
        <obo:IAO_0000115>A volcanic arc in the Andes of southwestern South America. It is one of the four volcanic zones of the Andes. The AVZ extends from the Chile Triple Junction to Tierra del Fuego archipelago, a distance of well over 1,000 km. The arc has formed due to subduction of the Antarctic Plate under the South American Plate. Between 49degS and 55degS.</obo:IAO_0000115>
        <oboInOwl:hasOBONamespace>GAZ</oboInOwl:hasOBONamespace>
        <oboInOwl:id>GAZ:00136454</oboInOwl:id>
        <rdfs:label>Austral Volcanic Zone</rdfs:label>
    </owl:NamedIndividual>
    


    <!-- http://purl.obolibrary.org/obo/GAZ_00136608 -->

    <owl:NamedIndividual rdf:about="http://purl.obolibrary.org/obo/GAZ_00136608">
        <obo:IAO_0000115>A reservoir located in the Andes, in the Santiago Metropolitan Region, Chile. It is formed by the damming of Yeso River, part of Maipo River basin.</obo:IAO_0000115>
        <oboInOwl:hasOBONamespace>GAZ</oboInOwl:hasOBONamespace>
        <oboInOwl:id>GAZ:00136608</oboInOwl:id>
        <rdfs:label>Embalse El Yeso</rdfs:label>
    </owl:NamedIndividual>
    


    <!-- http://purl.obolibrary.org/obo/GAZ_00136613 -->

    <owl:NamedIndividual rdf:about="http://purl.obolibrary.org/obo/GAZ_00136613">
        <obo:RO_0001025 rdf:resource="http://purl.obolibrary.org/obo/GAZ_00056452"/>
        <obo:IAO_0000115>Unas fuentes termales ubicadas en Chile, en la region de Los Lagos, ubicado a 80 km al este de la ciudad de Osorno.</obo:IAO_0000115>
        <oboInOwl:hasOBONamespace>GAZ</oboInOwl:hasOBONamespace>
        <oboInOwl:id>GAZ:00136613</oboInOwl:id>
        <rdfs:label>Termas de Aguas Calientes</rdfs:label>
    </owl:NamedIndividual>
    


    <!-- http://purl.obolibrary.org/obo/GAZ_00136671 -->

    <owl:NamedIndividual rdf:about="http://purl.obolibrary.org/obo/GAZ_00136671">
        <obo:RO_0001025 rdf:resource="http://purl.obolibrary.org/obo/GAZ_00136673"/>
        <obo:IAO_0000115>A Natural Monument located in the Chilean Patagonia, 24 km northwest of Puerto Natales and 270 km north of Punta Arenas. The monument is situated along the flanks of the Cerro Benitez Mountains. It comprises several caves and a rock formation called Silla del Diablo (Devil&apos;s Chair).</obo:IAO_0000115>
        <oboInOwl:hasOBONamespace>GAZ</oboInOwl:hasOBONamespace>
        <oboInOwl:id>GAZ:00136671</oboInOwl:id>
        <rdfs:label>Monumento Natural Cueva del Milodon</rdfs:label>
    </owl:NamedIndividual>
    


    <!-- http://purl.obolibrary.org/obo/GAZ_00136673 -->

    <owl:NamedIndividual rdf:about="http://purl.obolibrary.org/obo/GAZ_00136673">
        <rdf:type rdf:resource="http://purl.obolibrary.org/obo/ENVO_00000191"/>
        <obo:RO_0001025 rdf:resource="http://purl.obolibrary.org/obo/GAZ_00136454"/>
        <obo:IAO_0000115>A Cretaceous landform of the Magallanes Foreland the Patagonian region of southeastern Chile. The Cerro Toro is an element of the southern Andes Mountain Range.</obo:IAO_0000115>
        <oboInOwl:hasOBONamespace>GAZ</oboInOwl:hasOBONamespace>
        <oboInOwl:id>GAZ:00136673</oboInOwl:id>
        <rdfs:label>Cerro Toro</rdfs:label>
    </owl:NamedIndividual>
    


    <!-- http://purl.obolibrary.org/obo/GAZ_00136709 -->

    <owl:NamedIndividual rdf:about="http://purl.obolibrary.org/obo/GAZ_00136709">
        <obo:RO_0001025 rdf:resource="http://purl.obolibrary.org/obo/GAZ_00056548"/>
        <obo:IAO_0000115>A lake.</obo:IAO_0000115>
        <oboInOwl:hasOBONamespace>GAZ</oboInOwl:hasOBONamespace>
        <oboInOwl:id>GAZ:00136709</oboInOwl:id>
        <rdfs:label>Laguna Verde</rdfs:label>
    </owl:NamedIndividual>
    


    <!-- http://purl.obolibrary.org/obo/GAZ_00136710 -->

    <owl:NamedIndividual rdf:about="http://purl.obolibrary.org/obo/GAZ_00136710">
        <obo:RO_0001025 rdf:resource="http://purl.obolibrary.org/obo/GAZ_00056548"/>
        <obo:IAO_0000115>A lake.</obo:IAO_0000115>
        <oboInOwl:hasOBONamespace>GAZ</oboInOwl:hasOBONamespace>
        <oboInOwl:id>GAZ:00136710</oboInOwl:id>
        <rdfs:label>Laguna Malleco</rdfs:label>
    </owl:NamedIndividual>
    


    <!-- http://purl.obolibrary.org/obo/GAZ_00136711 -->

    <owl:NamedIndividual rdf:about="http://purl.obolibrary.org/obo/GAZ_00136711">
        <obo:RO_0001025 rdf:resource="http://purl.obolibrary.org/obo/GAZ_00056523"/>
        <obo:IAO_0000115>A lake.</obo:IAO_0000115>
        <oboInOwl:hasOBONamespace>GAZ</oboInOwl:hasOBONamespace>
        <oboInOwl:id>GAZ:00136711</oboInOwl:id>
        <rdfs:label>Laguna Quillelhue</rdfs:label>
    </owl:NamedIndividual>
    


    <!-- http://purl.obolibrary.org/obo/GAZ_00136712 -->

    <owl:NamedIndividual rdf:about="http://purl.obolibrary.org/obo/GAZ_00136712">
        <obo:RO_0001025 rdf:resource="http://purl.obolibrary.org/obo/GAZ_00056523"/>
        <obo:IAO_0000115>A lake.</obo:IAO_0000115>
        <oboInOwl:hasOBONamespace>GAZ</oboInOwl:hasOBONamespace>
        <oboInOwl:id>GAZ:00136712</oboInOwl:id>
        <rdfs:label>Laguna Huinfiuca</rdfs:label>
    </owl:NamedIndividual>
    


    <!-- http://purl.obolibrary.org/obo/GAZ_00136713 -->

    <owl:NamedIndividual rdf:about="http://purl.obolibrary.org/obo/GAZ_00136713">
        <obo:RO_0001025 rdf:resource="http://purl.obolibrary.org/obo/GAZ_00056523"/>
        <obo:IAO_0000115>A lake.</obo:IAO_0000115>
        <oboInOwl:hasOBONamespace>GAZ</oboInOwl:hasOBONamespace>
        <oboInOwl:id>GAZ:00136713</oboInOwl:id>
        <rdfs:label>Laguna de Los Patos</rdfs:label>
    </owl:NamedIndividual>
    


    <!-- http://purl.obolibrary.org/obo/GAZ_00136714 -->

    <owl:NamedIndividual rdf:about="http://purl.obolibrary.org/obo/GAZ_00136714">
        <obo:RO_0001025 rdf:resource="http://purl.obolibrary.org/obo/GAZ_00056523"/>
        <obo:IAO_0000115>A lake.</obo:IAO_0000115>
        <oboInOwl:hasOBONamespace>GAZ</oboInOwl:hasOBONamespace>
        <oboInOwl:id>GAZ:00136714</oboInOwl:id>
        <rdfs:label>Laguna Avutardas</rdfs:label>
    </owl:NamedIndividual>
    


    <!-- http://purl.obolibrary.org/obo/GAZ_00136715 -->

    <owl:NamedIndividual rdf:about="http://purl.obolibrary.org/obo/GAZ_00136715">
        <obo:RO_0001025 rdf:resource="http://purl.obolibrary.org/obo/GAZ_00056523"/>
        <obo:IAO_0000115>A lake.</obo:IAO_0000115>
        <oboInOwl:hasOBONamespace>GAZ</oboInOwl:hasOBONamespace>
        <oboInOwl:id>GAZ:00136715</oboInOwl:id>
        <rdfs:label>Laguna Azul</rdfs:label>
    </owl:NamedIndividual>
    


    <!-- http://purl.obolibrary.org/obo/GAZ_00136716 -->

    <owl:NamedIndividual rdf:about="http://purl.obolibrary.org/obo/GAZ_00136716">
        <obo:RO_0001025 rdf:resource="http://purl.obolibrary.org/obo/GAZ_00056523"/>
        <obo:IAO_0000115>A lake.</obo:IAO_0000115>
        <oboInOwl:hasOBONamespace>GAZ</oboInOwl:hasOBONamespace>
        <oboInOwl:id>GAZ:00136716</oboInOwl:id>
        <rdfs:label>Laguna Verde</rdfs:label>
    </owl:NamedIndividual>
    


    <!-- http://purl.obolibrary.org/obo/GAZ_00136717 -->

    <owl:NamedIndividual rdf:about="http://purl.obolibrary.org/obo/GAZ_00136717">
        <obo:RO_0001025 rdf:resource="http://purl.obolibrary.org/obo/GAZ_00056523"/>
        <obo:IAO_0000115>A lake.</obo:IAO_0000115>
        <oboInOwl:hasOBONamespace>GAZ</oboInOwl:hasOBONamespace>
        <oboInOwl:id>GAZ:00136717</oboInOwl:id>
        <rdfs:label>Laguna Blanca</rdfs:label>
    </owl:NamedIndividual>
    


    <!-- http://purl.obolibrary.org/obo/GAZ_00136729 -->

    <owl:NamedIndividual rdf:about="http://purl.obolibrary.org/obo/GAZ_00136729">
        <obo:RO_0001025 rdf:resource="http://purl.obolibrary.org/obo/GAZ_00056588"/>
        <obo:IAO_0000115>A glacier.</obo:IAO_0000115>
        <oboInOwl:hasOBONamespace>GAZ</oboInOwl:hasOBONamespace>
        <oboInOwl:id>GAZ:00136729</oboInOwl:id>
        <rdfs:label>Glaciar Aguila</rdfs:label>
    </owl:NamedIndividual>
    


    <!-- http://purl.obolibrary.org/obo/GAZ_00136730 -->

    <owl:NamedIndividual rdf:about="http://purl.obolibrary.org/obo/GAZ_00136730">
        <obo:RO_0001025 rdf:resource="http://purl.obolibrary.org/obo/GAZ_00056588"/>
        <obo:IAO_0000115>A glacier.</obo:IAO_0000115>
        <oboInOwl:hasOBONamespace>GAZ</oboInOwl:hasOBONamespace>
        <oboInOwl:id>GAZ:00136730</oboInOwl:id>
        <rdfs:label>Glaciar Garibaldi</rdfs:label>
    </owl:NamedIndividual>
    


    <!-- http://purl.obolibrary.org/obo/GAZ_00136731 -->

    <owl:NamedIndividual rdf:about="http://purl.obolibrary.org/obo/GAZ_00136731">
        <obo:RO_0001025 rdf:resource="http://purl.obolibrary.org/obo/GAZ_00056588"/>
        <obo:IAO_0000115>A tidewater glacier located in Alberto de Agostini National Park, Isla Grande de Tierra del Fuego. The glacier spills out from the backbone of the Cordillera Darwin and calves into Ainsworth Bay, an embayment of the Almirantazgo Fjord.</obo:IAO_0000115>
        <oboInOwl:hasOBONamespace>GAZ</oboInOwl:hasOBONamespace>
        <oboInOwl:id>GAZ:00136731</oboInOwl:id>
        <rdfs:label>Glaciar Marinelli</rdfs:label>
    </owl:NamedIndividual>
    


    <!-- http://purl.obolibrary.org/obo/GAZ_00136732 -->

    <owl:NamedIndividual rdf:about="http://purl.obolibrary.org/obo/GAZ_00136732">
        <obo:RO_0001025 rdf:resource="http://purl.obolibrary.org/obo/GAZ_00056588"/>
        <obo:IAO_0000115>A glacier.</obo:IAO_0000115>
        <oboInOwl:hasOBONamespace>GAZ</oboInOwl:hasOBONamespace>
        <oboInOwl:id>GAZ:00136732</oboInOwl:id>
        <rdfs:label>Glaciar Brookes</rdfs:label>
    </owl:NamedIndividual>
    


    <!-- http://purl.obolibrary.org/obo/GAZ_00136733 -->

    <owl:NamedIndividual rdf:about="http://purl.obolibrary.org/obo/GAZ_00136733">
        <obo:RO_0001025 rdf:resource="http://purl.obolibrary.org/obo/GAZ_00056588"/>
        <obo:IAO_0000115>A glacier.</obo:IAO_0000115>
        <oboInOwl:hasOBONamespace>GAZ</oboInOwl:hasOBONamespace>
        <oboInOwl:id>GAZ:00136733</oboInOwl:id>
        <rdfs:label>Glaciar Pia</rdfs:label>
    </owl:NamedIndividual>
    


    <!-- http://purl.obolibrary.org/obo/GAZ_00136734 -->

    <owl:NamedIndividual rdf:about="http://purl.obolibrary.org/obo/GAZ_00136734">
        <obo:RO_0001025 rdf:resource="http://purl.obolibrary.org/obo/GAZ_00056588"/>
        <obo:IAO_0000115>A glacier.</obo:IAO_0000115>
        <oboInOwl:hasOBONamespace>GAZ</oboInOwl:hasOBONamespace>
        <oboInOwl:id>GAZ:00136734</oboInOwl:id>
        <rdfs:label>Glaciar Italia</rdfs:label>
    </owl:NamedIndividual>
    


    <!-- http://purl.obolibrary.org/obo/GAZ_00136735 -->

    <owl:NamedIndividual rdf:about="http://purl.obolibrary.org/obo/GAZ_00136735">
        <obo:RO_0001025 rdf:resource="http://purl.obolibrary.org/obo/GAZ_00056588"/>
        <obo:IAO_0000115>A glacier.</obo:IAO_0000115>
        <oboInOwl:hasOBONamespace>GAZ</oboInOwl:hasOBONamespace>
        <oboInOwl:id>GAZ:00136735</oboInOwl:id>
        <rdfs:label>Glaciar Roncali</rdfs:label>
    </owl:NamedIndividual>
    


    <!-- http://purl.obolibrary.org/obo/GAZ_00136736 -->

    <owl:NamedIndividual rdf:about="http://purl.obolibrary.org/obo/GAZ_00136736">
        <obo:RO_0001025 rdf:resource="http://purl.obolibrary.org/obo/GAZ_00056588"/>
        <obo:IAO_0000115>A glacier.</obo:IAO_0000115>
        <oboInOwl:hasOBONamespace>GAZ</oboInOwl:hasOBONamespace>
        <oboInOwl:id>GAZ:00136736</oboInOwl:id>
        <rdfs:label>Glaciar Gunter Plushow</rdfs:label>
    </owl:NamedIndividual>
    


    <!-- http://purl.obolibrary.org/obo/GAZ_00136746 -->

    <owl:NamedIndividual rdf:about="http://purl.obolibrary.org/obo/GAZ_00136746">
        <obo:RO_0001025 rdf:resource="http://purl.obolibrary.org/obo/GAZ_00056517"/>
        <obo:IAO_0000115>Hot springs.</obo:IAO_0000115>
        <oboInOwl:hasOBONamespace>GAZ</oboInOwl:hasOBONamespace>
        <oboInOwl:id>GAZ:00136746</oboInOwl:id>
        <rdfs:label>Termas de Puchuldiza</rdfs:label>
    </owl:NamedIndividual>
    


    <!-- http://purl.obolibrary.org/obo/GAZ_00136773 -->

    <owl:NamedIndividual rdf:about="http://purl.obolibrary.org/obo/GAZ_00136773">
        <obo:RO_0001025 rdf:resource="http://purl.obolibrary.org/obo/GAZ_00136449"/>
        <obo:IAO_0000115>Un estratovolcan situado en la frontera de Chile con Argentina, cerca del paso fronteizo San Francico, entre la Region de Atacama y la Provincia de Catamarca.</obo:IAO_0000115>
        <oboInOwl:hasOBONamespace>GAZ</oboInOwl:hasOBONamespace>
        <oboInOwl:id>GAZ:00136773</oboInOwl:id>
        <rdfs:label>Volcan Los Patos</rdfs:label>
    </owl:NamedIndividual>
    


    <!-- http://purl.obolibrary.org/obo/GAZ_00136774 -->

    <owl:NamedIndividual rdf:about="http://purl.obolibrary.org/obo/GAZ_00136774">
        <obo:RO_0001025 rdf:resource="http://purl.obolibrary.org/obo/GAZ_00136449"/>
        <obo:IAO_0000115>Un estratovolcan situado en la Cordillera de los Andes, en el limite entre Argentina y Chile. Tiene una altura de 6,488 metros sobre el nivel del mar, y se encuentra ubicado entre la Region de Atacama y la Provincia de Catamarca. Forma parte de una larga cadena volcanica, junto otros grandes volcanes tales como el San Francisco, el Fraile, el Incahuasi, el Ojos del Salado, el Cerro Solo y el Tres Cruces.</obo:IAO_0000115>
        <oboInOwl:hasOBONamespace>GAZ</oboInOwl:hasOBONamespace>
        <oboInOwl:id>GAZ:00136774</oboInOwl:id>
        <rdfs:label>El Muerto</rdfs:label>
    </owl:NamedIndividual>
    


    <!-- http://purl.obolibrary.org/obo/GAZ_00136775 -->

    <owl:NamedIndividual rdf:about="http://purl.obolibrary.org/obo/GAZ_00136775">
        <obo:RO_0001025 rdf:resource="http://purl.obolibrary.org/obo/GAZ_00056494"/>
        <obo:RO_0001025 rdf:resource="http://purl.obolibrary.org/obo/GAZ_00136449"/>
        <obo:IAO_0000115>A mountain in the Andes Mountains. It has two main summits, Tres Cruces Sur at 6,749 m and Tres Cruces Central at 6,629 m and a third more minor summit, Tres Cruces Norte 6030m. The former marks the border between Argentina and Chile.</obo:IAO_0000115>
        <oboInOwl:hasOBONamespace>GAZ</oboInOwl:hasOBONamespace>
        <oboInOwl:id>GAZ:00136775</oboInOwl:id>
        <rdfs:label>Nevado Tres Cruces</rdfs:label>
    </owl:NamedIndividual>
    


    <!-- http://purl.obolibrary.org/obo/GAZ_00137593 -->

    <owl:NamedIndividual rdf:about="http://purl.obolibrary.org/obo/GAZ_00137593">
        <obo:RO_0001025 rdf:resource="http://purl.obolibrary.org/obo/GAZ_00056728"/>
        <obo:IAO_0000115>A crater lake. Se encuentra al pie de la ladera noroeste del Volcan Tromen a una altura sobre el nivel del mar de 2,100 m y cubre una superficie aproximada de 4 km2.</obo:IAO_0000115>
        <oboInOwl:hasOBONamespace>GAZ</oboInOwl:hasOBONamespace>
        <oboInOwl:id>GAZ:00137593</oboInOwl:id>
        <rdfs:label>Laguna Tromen</rdfs:label>
    </owl:NamedIndividual>
    


    <!-- http://purl.obolibrary.org/obo/GAZ_00138615 -->

    <owl:NamedIndividual rdf:about="http://purl.obolibrary.org/obo/GAZ_00138615">
        <obo:RO_0001025 rdf:resource="http://purl.obolibrary.org/obo/GAZ_00136448"/>
        <oboInOwl:hasOBONamespace>GAZ</oboInOwl:hasOBONamespace>
        <oboInOwl:id>GAZ:00138615</oboInOwl:id>
        <rdfs:label>Volcan Chinibano</rdfs:label>
    </owl:NamedIndividual>
    


    <!-- http://purl.obolibrary.org/obo/GAZ_00138616 -->

    <owl:NamedIndividual rdf:about="http://purl.obolibrary.org/obo/GAZ_00138616">
        <obo:RO_0001025 rdf:resource="http://purl.obolibrary.org/obo/GAZ_00136448"/>
        <oboInOwl:hasOBONamespace>GAZ</oboInOwl:hasOBONamespace>
        <oboInOwl:id>GAZ:00138616</oboInOwl:id>
        <rdfs:label>Volcan Igualata</rdfs:label>
    </owl:NamedIndividual>
    


    <!-- http://purl.obolibrary.org/obo/GAZ_00138617 -->

    <owl:NamedIndividual rdf:about="http://purl.obolibrary.org/obo/GAZ_00138617">
        <obo:RO_0001025 rdf:resource="http://purl.obolibrary.org/obo/GAZ_00056699"/>
        <oboInOwl:hasOBONamespace>GAZ</oboInOwl:hasOBONamespace>
        <oboInOwl:id>GAZ:00138617</oboInOwl:id>
        <rdfs:label>Volcan Taapaca</rdfs:label>
    </owl:NamedIndividual>
    


    <!-- http://purl.obolibrary.org/obo/GAZ_00138618 -->

    <owl:NamedIndividual rdf:about="http://purl.obolibrary.org/obo/GAZ_00138618">
        <rdf:type rdf:resource="http://purl.obolibrary.org/obo/ENVO_00000354"/>
        <obo:RO_0001025 rdf:resource="http://purl.obolibrary.org/obo/GAZ_00136449"/>
        <obo:IAO_0000115>A volcanic system.</obo:IAO_0000115>
        <oboInOwl:hasOBONamespace>GAZ</oboInOwl:hasOBONamespace>
        <oboInOwl:id>GAZ:00138618</oboInOwl:id>
        <rdfs:label>Pastos Grandes Caldera</rdfs:label>
    </owl:NamedIndividual>
    


    <!-- http://purl.obolibrary.org/obo/GAZ_00138619 -->

    <owl:NamedIndividual rdf:about="http://purl.obolibrary.org/obo/GAZ_00138619">
        <obo:RO_0001025 rdf:resource="http://purl.obolibrary.org/obo/GAZ_00136449"/>
        <oboInOwl:hasOBONamespace>GAZ</oboInOwl:hasOBONamespace>
        <oboInOwl:id>GAZ:00138619</oboInOwl:id>
        <rdfs:label>Cerro Panizos</rdfs:label>
    </owl:NamedIndividual>
    


    <!-- http://purl.obolibrary.org/obo/GAZ_00138620 -->

    <owl:NamedIndividual rdf:about="http://purl.obolibrary.org/obo/GAZ_00138620">
        <rdf:type rdf:resource="http://purl.obolibrary.org/obo/ENVO_00000354"/>
        <obo:RO_0001025 rdf:resource="http://purl.obolibrary.org/obo/GAZ_00136449"/>
        <obo:IAO_0000115>A volcanic system.</obo:IAO_0000115>
        <oboInOwl:hasOBONamespace>GAZ</oboInOwl:hasOBONamespace>
        <oboInOwl:id>GAZ:00138620</oboInOwl:id>
        <rdfs:label>Altiplano-Puna Volcanic Complex</rdfs:label>
    </owl:NamedIndividual>
    


    <!-- http://purl.obolibrary.org/obo/GAZ_00138621 -->

    <owl:NamedIndividual rdf:about="http://purl.obolibrary.org/obo/GAZ_00138621">
        <rdf:type rdf:resource="http://purl.obolibrary.org/obo/ENVO_00000354"/>
        <obo:RO_0001025 rdf:resource="http://purl.obolibrary.org/obo/GAZ_00136449"/>
        <obo:IAO_0000115>A volcanic system.</obo:IAO_0000115>
        <oboInOwl:hasOBONamespace>GAZ</oboInOwl:hasOBONamespace>
        <oboInOwl:id>GAZ:00138621</oboInOwl:id>
        <rdfs:label>Cerro Guacha</rdfs:label>
    </owl:NamedIndividual>
    


    <!-- http://purl.obolibrary.org/obo/GAZ_00138622 -->

    <owl:NamedIndividual rdf:about="http://purl.obolibrary.org/obo/GAZ_00138622">
        <rdf:type rdf:resource="http://purl.obolibrary.org/obo/ENVO_00000354"/>
        <obo:RO_0001025 rdf:resource="http://purl.obolibrary.org/obo/GAZ_00136449"/>
        <obo:IAO_0000115>A volcanic system.</obo:IAO_0000115>
        <oboInOwl:hasOBONamespace>GAZ</oboInOwl:hasOBONamespace>
        <oboInOwl:id>GAZ:00138622</oboInOwl:id>
        <rdfs:label>La Pacana Caldera</rdfs:label>
    </owl:NamedIndividual>
    


    <!-- http://purl.obolibrary.org/obo/GAZ_00138623 -->

    <owl:NamedIndividual rdf:about="http://purl.obolibrary.org/obo/GAZ_00138623">
        <obo:RO_0001025 rdf:resource="http://purl.obolibrary.org/obo/GAZ_00136449"/>
        <obo:IAO_0000115>A caldera complex.</obo:IAO_0000115>
        <oboInOwl:hasOBONamespace>GAZ</oboInOwl:hasOBONamespace>
        <oboInOwl:id>GAZ:00138623</oboInOwl:id>
        <rdfs:label>Incapillo</rdfs:label>
    </owl:NamedIndividual>
    


    <!-- http://purl.obolibrary.org/obo/GAZ_00138624 -->

    <owl:NamedIndividual rdf:about="http://purl.obolibrary.org/obo/GAZ_00138624">
        <obo:RO_0001025 rdf:resource="http://purl.obolibrary.org/obo/GAZ_00136449"/>
        <obo:IAO_0000115>A volcano in the north of the province of La Rioja, Argentina, near the provincial border with Catamarca.</obo:IAO_0000115>
        <oboInOwl:hasOBONamespace>GAZ</oboInOwl:hasOBONamespace>
        <oboInOwl:id>GAZ:00138624</oboInOwl:id>
        <rdfs:label>Cerro Bonete</rdfs:label>
    </owl:NamedIndividual>
    


    <!-- http://purl.obolibrary.org/obo/GAZ_00138625 -->

    <owl:NamedIndividual rdf:about="http://purl.obolibrary.org/obo/GAZ_00138625">
        <obo:RO_0001025 rdf:resource="http://purl.obolibrary.org/obo/GAZ_00136453"/>
        <oboInOwl:hasOBONamespace>GAZ</oboInOwl:hasOBONamespace>
        <oboInOwl:id>GAZ:00138625</oboInOwl:id>
        <rdfs:label>Caviahue Caldera Complex</rdfs:label>
    </owl:NamedIndividual>
    


    <!-- http://purl.obolibrary.org/obo/GAZ_00138790 -->

    <owl:NamedIndividual rdf:about="http://purl.obolibrary.org/obo/GAZ_00138790">
        <obo:RO_0001025 rdf:resource="http://purl.obolibrary.org/obo/GAZ_00056484"/>
        <obo:IAO_0000115>A major vent on the northern flank of Cerro Azul.</obo:IAO_0000115>
        <oboInOwl:hasOBONamespace>GAZ</oboInOwl:hasOBONamespace>
        <oboInOwl:id>GAZ:00138790</oboInOwl:id>
        <rdfs:label>Volcan Quizapu</rdfs:label>
    </owl:NamedIndividual>
    


    <!-- http://purl.obolibrary.org/obo/GAZ_00138791 -->

    <owl:NamedIndividual rdf:about="http://purl.obolibrary.org/obo/GAZ_00138791">
        <obo:RO_0001025 rdf:resource="http://purl.obolibrary.org/obo/GAZ_00136453"/>
        <oboInOwl:hasOBONamespace>GAZ</oboInOwl:hasOBONamespace>
        <oboInOwl:id>GAZ:00138791</oboInOwl:id>
        <rdfs:label>Pino Hachado Volcanic Complex</rdfs:label>
    </owl:NamedIndividual>
    


    <!-- http://purl.obolibrary.org/obo/GAZ_00138792 -->

    <owl:NamedIndividual rdf:about="http://purl.obolibrary.org/obo/GAZ_00138792">
        <obo:RO_0001025 rdf:resource="http://purl.obolibrary.org/obo/GAZ_00056519"/>
        <obo:IAO_0000115>A lake.</obo:IAO_0000115>
        <oboInOwl:hasOBONamespace>GAZ</oboInOwl:hasOBONamespace>
        <oboInOwl:id>GAZ:00138792</oboInOwl:id>
        <rdfs:label>Lago Paimun</rdfs:label>
    </owl:NamedIndividual>
    


    <!-- http://purl.obolibrary.org/obo/GAZ_00138793 -->

    <owl:NamedIndividual rdf:about="http://purl.obolibrary.org/obo/GAZ_00138793">
        <obo:RO_0001025 rdf:resource="http://purl.obolibrary.org/obo/GAZ_00056519"/>
        <obo:IAO_0000115>Un lago ubicado en el sudeste de la provincia del Neuquen, en el sur de la Republica Argentina. En realidad, se trata de dos lagos, muy cercanos uno del otro: el Curruhue Grande, aguas arriba, y el Curruhue Chico, ubicado aguas abajo del primero.</obo:IAO_0000115>
        <oboInOwl:hasOBONamespace>GAZ</oboInOwl:hasOBONamespace>
        <oboInOwl:id>GAZ:00138793</oboInOwl:id>
        <rdfs:label>Lago Curruhue</rdfs:label>
    </owl:NamedIndividual>
    


    <!-- http://purl.obolibrary.org/obo/GAZ_00138794 -->

    <owl:NamedIndividual rdf:about="http://purl.obolibrary.org/obo/GAZ_00138794">
        <obo:RO_0001025 rdf:resource="http://purl.obolibrary.org/obo/GAZ_00138793"/>
        <obo:IAO_0000115>The smaller of the two Curruhue Lakes.</obo:IAO_0000115>
        <oboInOwl:hasOBONamespace>GAZ</oboInOwl:hasOBONamespace>
        <oboInOwl:id>GAZ:00138794</oboInOwl:id>
        <rdfs:label>Lago Curruhue Chico</rdfs:label>
    </owl:NamedIndividual>
    


    <!-- http://purl.obolibrary.org/obo/GAZ_00138795 -->

    <owl:NamedIndividual rdf:about="http://purl.obolibrary.org/obo/GAZ_00138795">
        <obo:RO_0001025 rdf:resource="http://purl.obolibrary.org/obo/GAZ_00138793"/>
        <obo:IAO_0000115>The larger of the two Curruhue Lakes.</obo:IAO_0000115>
        <oboInOwl:hasOBONamespace>GAZ</oboInOwl:hasOBONamespace>
        <oboInOwl:id>GAZ:00138795</oboInOwl:id>
        <rdfs:label>Lago Curruhue Grande</rdfs:label>
    </owl:NamedIndividual>
    


    <!-- http://purl.obolibrary.org/obo/GAZ_00138796 -->

    <owl:NamedIndividual rdf:about="http://purl.obolibrary.org/obo/GAZ_00138796">
        <obo:RO_0001025 rdf:resource="http://purl.obolibrary.org/obo/GAZ_00056519"/>
        <obo:IAO_0000115>A lake. Esta ubicado en el sudeste de la provincia del Neuquen, en el sur de la Republica Argentina.</obo:IAO_0000115>
        <oboInOwl:hasOBONamespace>GAZ</oboInOwl:hasOBONamespace>
        <oboInOwl:id>GAZ:00138796</oboInOwl:id>
        <rdfs:label>Lago Meliquina</rdfs:label>
    </owl:NamedIndividual>
    


    <!-- http://purl.obolibrary.org/obo/GAZ_00138797 -->

    <owl:NamedIndividual rdf:about="http://purl.obolibrary.org/obo/GAZ_00138797">
        <obo:RO_0001025 rdf:resource="http://purl.obolibrary.org/obo/GAZ_00056519"/>
        <obo:IAO_0000115>Un lago ubicado en el sudeste de la provincia del Neuquen, en el sur de la Republica Argentina.</obo:IAO_0000115>
        <oboInOwl:hasOBONamespace>GAZ</oboInOwl:hasOBONamespace>
        <oboInOwl:id>GAZ:00138797</oboInOwl:id>
        <rdfs:label>Lago Lolog</rdfs:label>
    </owl:NamedIndividual>
    


    <!-- http://purl.obolibrary.org/obo/GAZ_00138798 -->

    <owl:NamedIndividual rdf:about="http://purl.obolibrary.org/obo/GAZ_00138798">
        <obo:RO_0001025 rdf:resource="http://purl.obolibrary.org/obo/GAZ_00056417"/>
        <obo:IAO_0000115>A stratovolcano.</obo:IAO_0000115>
        <oboInOwl:hasOBONamespace>GAZ</oboInOwl:hasOBONamespace>
        <oboInOwl:id>GAZ:00138798</oboInOwl:id>
        <rdfs:label>Cerro Uquila</rdfs:label>
    </owl:NamedIndividual>
    


    <!-- http://purl.obolibrary.org/obo/GAZ_00138799 -->

    <owl:NamedIndividual rdf:about="http://purl.obolibrary.org/obo/GAZ_00138799">
        <obo:RO_0001025 rdf:resource="http://purl.obolibrary.org/obo/GAZ_00056417"/>
        <obo:IAO_0000115>A stratovolcano.</obo:IAO_0000115>
        <oboInOwl:hasOBONamespace>GAZ</oboInOwl:hasOBONamespace>
        <oboInOwl:id>GAZ:00138799</oboInOwl:id>
        <rdfs:label>Cerro Luxsar</rdfs:label>
    </owl:NamedIndividual>
    


    <!-- http://purl.obolibrary.org/obo/GAZ_00138800 -->

    <owl:NamedIndividual rdf:about="http://purl.obolibrary.org/obo/GAZ_00138800">
        <obo:RO_0001025 rdf:resource="http://purl.obolibrary.org/obo/GAZ_00056423"/>
        <obo:IAO_0000115>A stratovolcano.</obo:IAO_0000115>
        <oboInOwl:hasOBONamespace>GAZ</oboInOwl:hasOBONamespace>
        <oboInOwl:id>GAZ:00138800</oboInOwl:id>
        <rdfs:label>El Apagado</rdfs:label>
    </owl:NamedIndividual>
    


    <!-- http://purl.obolibrary.org/obo/GAZ_00138801 -->

    <owl:NamedIndividual rdf:about="http://purl.obolibrary.org/obo/GAZ_00138801">
        <obo:RO_0001025 rdf:resource="http://purl.obolibrary.org/obo/GAZ_00056423"/>
        <obo:IAO_0000115>A stratovolcano.</obo:IAO_0000115>
        <oboInOwl:hasOBONamespace>GAZ</oboInOwl:hasOBONamespace>
        <oboInOwl:id>GAZ:00138801</oboInOwl:id>
        <rdfs:label>Cerro Curiquinca</rdfs:label>
    </owl:NamedIndividual>
    


    <!-- http://purl.obolibrary.org/obo/GAZ_00138802 -->

    <owl:NamedIndividual rdf:about="http://purl.obolibrary.org/obo/GAZ_00138802">
        <obo:RO_0001025 rdf:resource="http://purl.obolibrary.org/obo/GAZ_00056423"/>
        <obo:IAO_0000115>A volcanic cone.</obo:IAO_0000115>
        <oboInOwl:hasOBONamespace>GAZ</oboInOwl:hasOBONamespace>
        <oboInOwl:id>GAZ:00138802</oboInOwl:id>
        <rdfs:label>Cerro Colorado</rdfs:label>
    </owl:NamedIndividual>
    


    <!-- http://purl.obolibrary.org/obo/GAZ_00138803 -->

    <owl:NamedIndividual rdf:about="http://purl.obolibrary.org/obo/GAZ_00138803">
        <obo:RO_0001025 rdf:resource="http://purl.obolibrary.org/obo/GAZ_00056254"/>
        <obo:RO_0001025 rdf:resource="http://purl.obolibrary.org/obo/GAZ_00089671"/>
        <obo:RO_0001025 rdf:resource="http://purl.obolibrary.org/obo/GAZ_00136448"/>
        <obo:IAO_0000115>Un nevado ubicado en la Cordillera Central, en los Andes colombianos, dentro del Parque Nacional de los Nevados.</obo:IAO_0000115>
        <oboInOwl:hasOBONamespace>GAZ</oboInOwl:hasOBONamespace>
        <oboInOwl:id>GAZ:00138803</oboInOwl:id>
        <rdfs:label>Nevado el Cisne</rdfs:label>
    </owl:NamedIndividual>
    


    <!-- http://purl.obolibrary.org/obo/GAZ_00138805 -->

    <owl:NamedIndividual rdf:about="http://purl.obolibrary.org/obo/GAZ_00138805">
        <obo:RO_0001025 rdf:resource="http://purl.obolibrary.org/obo/GAZ_00089671"/>
        <obo:IAO_0000115>A lake.</obo:IAO_0000115>
        <oboInOwl:hasOBONamespace>GAZ</oboInOwl:hasOBONamespace>
        <oboInOwl:id>GAZ:00138805</oboInOwl:id>
        <rdfs:label>Laguna La Leona</rdfs:label>
    </owl:NamedIndividual>
    


    <!-- http://purl.obolibrary.org/obo/GAZ_00138806 -->

    <owl:NamedIndividual rdf:about="http://purl.obolibrary.org/obo/GAZ_00138806">
        <obo:RO_0001025 rdf:resource="http://purl.obolibrary.org/obo/GAZ_00089671"/>
        <obo:IAO_0000115>A lake.</obo:IAO_0000115>
        <oboInOwl:hasOBONamespace>GAZ</oboInOwl:hasOBONamespace>
        <oboInOwl:id>GAZ:00138806</oboInOwl:id>
        <rdfs:label>Laguna Verde</rdfs:label>
    </owl:NamedIndividual>
    


    <!-- http://purl.obolibrary.org/obo/GAZ_00138807 -->

    <owl:NamedIndividual rdf:about="http://purl.obolibrary.org/obo/GAZ_00138807">
        <obo:RO_0001025 rdf:resource="http://purl.obolibrary.org/obo/GAZ_00089671"/>
        <obo:IAO_0000115>A lake.</obo:IAO_0000115>
        <oboInOwl:hasOBONamespace>GAZ</oboInOwl:hasOBONamespace>
        <oboInOwl:id>GAZ:00138807</oboInOwl:id>
        <rdfs:label>Laguna Negra</rdfs:label>
    </owl:NamedIndividual>
    


    <!-- http://purl.obolibrary.org/obo/GAZ_00138859 -->

    <owl:NamedIndividual rdf:about="http://purl.obolibrary.org/obo/GAZ_00138859">
        <obo:RO_0001025 rdf:resource="http://purl.obolibrary.org/obo/GAZ_00056508"/>
        <oboInOwl:hasOBONamespace>GAZ</oboInOwl:hasOBONamespace>
        <oboInOwl:id>GAZ:00138859</oboInOwl:id>
        <rdfs:label>Volcan la Moyra</rdfs:label>
    </owl:NamedIndividual>
    


    <!-- http://purl.obolibrary.org/obo/GAZ_00139014 -->

    <owl:NamedIndividual rdf:about="http://purl.obolibrary.org/obo/GAZ_00139014">
        <obo:RO_0001025 rdf:resource="http://purl.obolibrary.org/obo/GAZ_00056519"/>
        <obo:IAO_0000115>Un lago de origen glaciario ubicado en la provincia del Neuquen, Argentina, en el departamento Alumine.</obo:IAO_0000115>
        <oboInOwl:hasOBONamespace>GAZ</oboInOwl:hasOBONamespace>
        <oboInOwl:id>GAZ:00139014</oboInOwl:id>
        <rdfs:label>Lago Quillen</rdfs:label>
    </owl:NamedIndividual>
    


    <!-- http://purl.obolibrary.org/obo/GAZ_00139015 -->

    <owl:NamedIndividual rdf:about="http://purl.obolibrary.org/obo/GAZ_00139015">
        <obo:RO_0001025 rdf:resource="http://purl.obolibrary.org/obo/GAZ_00056519"/>
        <obo:IAO_0000115>Un espejo de agua en la provincia de Neuquen, de alrededor de 5,300 ha, cuya costa sur pertenece al Parque Nacional Lanin.</obo:IAO_0000115>
        <oboInOwl:hasOBONamespace>GAZ</oboInOwl:hasOBONamespace>
        <oboInOwl:id>GAZ:00139015</oboInOwl:id>
        <rdfs:label>Lago Norquinco</rdfs:label>
    </owl:NamedIndividual>
    


    <!-- http://purl.obolibrary.org/obo/GAZ_00139043 -->

    <owl:NamedIndividual rdf:about="http://purl.obolibrary.org/obo/GAZ_00139043">
        <obo:RO_0001025 rdf:resource="http://purl.obolibrary.org/obo/GAZ_00056519"/>
        <obo:IAO_0000115>Un espejo lacustre de origen glaciar situado en las estribaciones orientales de los Andes, en la provincia del Neuquen, en el Suroeste de Argentina. Es parte del Parque Nacional Lanin.</obo:IAO_0000115>
        <oboInOwl:hasOBONamespace>GAZ</oboInOwl:hasOBONamespace>
        <oboInOwl:id>GAZ:00139043</oboInOwl:id>
        <rdfs:label>Lago Carilafquen</rdfs:label>
    </owl:NamedIndividual>
    


    <!-- http://purl.obolibrary.org/obo/GAZ_00139044 -->

    <owl:NamedIndividual rdf:about="http://purl.obolibrary.org/obo/GAZ_00139044">
        <obo:RO_0001025 rdf:resource="http://purl.obolibrary.org/obo/GAZ_00056519"/>
        <obo:IAO_0000115>A lake. Ubicado en la provincia del Neuquen, en el sur de la Republica Argentina, en plena Cordillera de los Andes. Esta separado del Lago Huechulafquen, del cual es tributario, por un corto estrecho.</obo:IAO_0000115>
        <oboInOwl:hasOBONamespace>GAZ</oboInOwl:hasOBONamespace>
        <oboInOwl:id>GAZ:00139044</oboInOwl:id>
        <rdfs:label>Lago Epulafquen</rdfs:label>
    </owl:NamedIndividual>
    


    <!-- http://purl.obolibrary.org/obo/GAZ_00139065 -->

    <owl:NamedIndividual rdf:about="http://purl.obolibrary.org/obo/GAZ_00139065">
        <obo:RO_0001025 rdf:resource="http://purl.obolibrary.org/obo/GAZ_00056519"/>
        <obo:IAO_0000115>Un espejo de agua ubicado en el Parque Nacional Lanin, en la zona cordillerana de la provincia de Neuquen, en el sur de la Argentina.</obo:IAO_0000115>
        <oboInOwl:hasOBONamespace>GAZ</oboInOwl:hasOBONamespace>
        <oboInOwl:id>GAZ:00139065</oboInOwl:id>
        <rdfs:label>Lago Tromen</rdfs:label>
    </owl:NamedIndividual>
    


    <!-- http://purl.obolibrary.org/obo/GAZ_00139108 -->

    <owl:NamedIndividual rdf:about="http://purl.obolibrary.org/obo/GAZ_00139108">
        <obo:RO_0001025 rdf:resource="http://purl.obolibrary.org/obo/GAZ_00056457"/>
        <obo:IAO_0000115>Un pequeno glaciar ubicado sobre el lado argentino del cerro Tronador, dentro del Parque Nacional Nahuel Huapi.</obo:IAO_0000115>
        <oboInOwl:hasOBONamespace>GAZ</oboInOwl:hasOBONamespace>
        <oboInOwl:id>GAZ:00139108</oboInOwl:id>
        <rdfs:label>Glaciar Castano Overo</rdfs:label>
    </owl:NamedIndividual>
    


    <!-- http://purl.obolibrary.org/obo/GAZ_00139109 -->

    <owl:NamedIndividual rdf:about="http://purl.obolibrary.org/obo/GAZ_00139109">
        <obo:RO_0001025 rdf:resource="http://purl.obolibrary.org/obo/GAZ_00056457"/>
        <obo:IAO_0000115>Uno de los diez glaciares que ocupan la cumbre del cerro Tronador, en San Carlos de Bariloche, en la provincia de Rio Negro, Argentina.</obo:IAO_0000115>
        <oboInOwl:hasOBONamespace>GAZ</oboInOwl:hasOBONamespace>
        <oboInOwl:id>GAZ:00139109</oboInOwl:id>
        <rdfs:label>Ventisquero Negro</rdfs:label>
    </owl:NamedIndividual>
    


    <!-- http://purl.obolibrary.org/obo/GAZ_00144444 -->

    <owl:NamedIndividual rdf:about="http://purl.obolibrary.org/obo/GAZ_00144444">
        <obo:RO_0001025 rdf:resource="http://purl.obolibrary.org/obo/GAZ_00051744"/>
        <obo:IAO_0000115>An island on the Aves de Barlovento reef.</obo:IAO_0000115>
        <oboInOwl:hasOBONamespace>GAZ</oboInOwl:hasOBONamespace>
        <oboInOwl:id>GAZ:00144444</oboInOwl:id>
        <rdfs:label>Isla Tesoro</rdfs:label>
    </owl:NamedIndividual>
    


    <!-- http://purl.obolibrary.org/obo/GAZ_00144445 -->

    <owl:NamedIndividual rdf:about="http://purl.obolibrary.org/obo/GAZ_00144445">
        <obo:RO_0001025 rdf:resource="http://purl.obolibrary.org/obo/GAZ_00051744"/>
        <obo:IAO_0000115>An island on the Aves de Barlovento reef.</obo:IAO_0000115>
        <oboInOwl:hasOBONamespace>GAZ</oboInOwl:hasOBONamespace>
        <oboInOwl:id>GAZ:00144445</oboInOwl:id>
        <rdfs:label>Isla Aves de Barlovento</rdfs:label>
    </owl:NamedIndividual>
    


    <!-- http://purl.obolibrary.org/obo/GAZ_00144446 -->

    <owl:NamedIndividual rdf:about="http://purl.obolibrary.org/obo/GAZ_00144446">
        <obo:RO_0001025 rdf:resource="http://purl.obolibrary.org/obo/GAZ_00051744"/>
        <obo:IAO_0000115>An island on the Aves de Barlovento reef.</obo:IAO_0000115>
        <oboInOwl:hasOBONamespace>GAZ</oboInOwl:hasOBONamespace>
        <oboInOwl:id>GAZ:00144446</oboInOwl:id>
        <rdfs:label>Cayo de Las Bobas</rdfs:label>
    </owl:NamedIndividual>
    


    <!-- http://purl.obolibrary.org/obo/GAZ_00144447 -->

    <owl:NamedIndividual rdf:about="http://purl.obolibrary.org/obo/GAZ_00144447">
        <obo:RO_0001025 rdf:resource="http://purl.obolibrary.org/obo/GAZ_00051744"/>
        <obo:IAO_0000115>An island on the Aves de Barlovento reef.</obo:IAO_0000115>
        <oboInOwl:hasOBONamespace>GAZ</oboInOwl:hasOBONamespace>
        <oboInOwl:id>GAZ:00144447</oboInOwl:id>
        <rdfs:label>Cayo Bubi</rdfs:label>
    </owl:NamedIndividual>
    


    <!-- http://purl.obolibrary.org/obo/GAZ_00144448 -->

    <owl:NamedIndividual rdf:about="http://purl.obolibrary.org/obo/GAZ_00144448">
        <obo:RO_0001025 rdf:resource="http://purl.obolibrary.org/obo/GAZ_00051743"/>
        <obo:IAO_0000115>An island on the Aves de Sotavento reef.</obo:IAO_0000115>
        <oboInOwl:hasOBONamespace>GAZ</oboInOwl:hasOBONamespace>
        <oboInOwl:id>GAZ:00144448</oboInOwl:id>
        <rdfs:label>Isla Larga</rdfs:label>
    </owl:NamedIndividual>
    


    <!-- http://purl.obolibrary.org/obo/GAZ_00144449 -->

    <owl:NamedIndividual rdf:about="http://purl.obolibrary.org/obo/GAZ_00144449">
        <obo:RO_0001025 rdf:resource="http://purl.obolibrary.org/obo/GAZ_00051743"/>
        <obo:IAO_0000115>An island on the Aves de Sotavento reef.</obo:IAO_0000115>
        <oboInOwl:hasOBONamespace>GAZ</oboInOwl:hasOBONamespace>
        <oboInOwl:id>GAZ:00144449</oboInOwl:id>
        <rdfs:label>Isla Aves de Sotavento</rdfs:label>
    </owl:NamedIndividual>
    


    <!-- http://purl.obolibrary.org/obo/GAZ_00144450 -->

    <owl:NamedIndividual rdf:about="http://purl.obolibrary.org/obo/GAZ_00144450">
        <obo:RO_0001025 rdf:resource="http://purl.obolibrary.org/obo/GAZ_00051743"/>
        <obo:IAO_0000115>An island on the Aves de Sotavento reef.</obo:IAO_0000115>
        <oboInOwl:hasOBONamespace>GAZ</oboInOwl:hasOBONamespace>
        <oboInOwl:id>GAZ:00144450</oboInOwl:id>
        <rdfs:label>Cayo Sterna</rdfs:label>
    </owl:NamedIndividual>
    


    <!-- http://purl.obolibrary.org/obo/GAZ_00144451 -->

    <owl:NamedIndividual rdf:about="http://purl.obolibrary.org/obo/GAZ_00144451">
        <obo:RO_0001025 rdf:resource="http://purl.obolibrary.org/obo/GAZ_00051743"/>
        <obo:IAO_0000115>An island on the Aves de Sotavento reef.</obo:IAO_0000115>
        <oboInOwl:hasOBONamespace>GAZ</oboInOwl:hasOBONamespace>
        <oboInOwl:id>GAZ:00144451</oboInOwl:id>
        <rdfs:label>Isla Maceta</rdfs:label>
    </owl:NamedIndividual>
    


    <!-- http://purl.obolibrary.org/obo/GAZ_00144452 -->

    <owl:NamedIndividual rdf:about="http://purl.obolibrary.org/obo/GAZ_00144452">
        <obo:RO_0001025 rdf:resource="http://purl.obolibrary.org/obo/GAZ_00051743"/>
        <obo:IAO_0000115>An island on the Aves de Sotavento reef.</obo:IAO_0000115>
        <oboInOwl:hasOBONamespace>GAZ</oboInOwl:hasOBONamespace>
        <oboInOwl:id>GAZ:00144452</oboInOwl:id>
        <rdfs:label>Cayos de La Colonia</rdfs:label>
    </owl:NamedIndividual>
    


    <!-- http://purl.obolibrary.org/obo/GAZ_00144453 -->

    <owl:NamedIndividual rdf:about="http://purl.obolibrary.org/obo/GAZ_00144453">
        <obo:RO_0001025 rdf:resource="http://purl.obolibrary.org/obo/GAZ_00051743"/>
        <obo:IAO_0000115>An island on the Aves de Sotavento reef.</obo:IAO_0000115>
        <oboInOwl:hasOBONamespace>GAZ</oboInOwl:hasOBONamespace>
        <oboInOwl:id>GAZ:00144453</oboInOwl:id>
        <rdfs:label>Isla Saquisaqui</rdfs:label>
    </owl:NamedIndividual>
    


    <!-- http://purl.obolibrary.org/obo/GAZ_00144454 -->

    <owl:NamedIndividual rdf:about="http://purl.obolibrary.org/obo/GAZ_00144454">
        <obo:RO_0001025 rdf:resource="http://purl.obolibrary.org/obo/GAZ_00051743"/>
        <obo:IAO_0000115>An island on the Aves de Sotavento reef.</obo:IAO_0000115>
        <oboInOwl:hasOBONamespace>GAZ</oboInOwl:hasOBONamespace>
        <oboInOwl:id>GAZ:00144454</oboInOwl:id>
        <rdfs:label>Cayo Tirra</rdfs:label>
    </owl:NamedIndividual>
    


    <!-- http://purl.obolibrary.org/obo/GAZ_00144833 -->

    <owl:NamedIndividual rdf:about="http://purl.obolibrary.org/obo/GAZ_00144833">
        <obo:RO_0001025 rdf:resource="http://purl.obolibrary.org/obo/GAZ_00047116"/>
        <obo:IAO_0000115>A lagoon.</obo:IAO_0000115>
        <oboInOwl:hasOBONamespace>GAZ</oboInOwl:hasOBONamespace>
        <oboInOwl:id>GAZ:00144833</oboInOwl:id>
        <rdfs:label>La Restintiga</rdfs:label>
    </owl:NamedIndividual>
    


    <!-- http://purl.obolibrary.org/obo/GAZ_00144840 -->

    <owl:NamedIndividual rdf:about="http://purl.obolibrary.org/obo/GAZ_00144840">
        <obo:RO_0001025 rdf:resource="http://purl.obolibrary.org/obo/GAZ_00056493"/>
        <obo:IAO_0000115>An acid crater lake.</obo:IAO_0000115>
        <oboInOwl:hasOBONamespace>GAZ</oboInOwl:hasOBONamespace>
        <oboInOwl:id>GAZ:00144840</oboInOwl:id>
        <rdfs:label>Copahue Crater Lake</rdfs:label>
    </owl:NamedIndividual>
    


    <!-- http://purl.obolibrary.org/obo/GAZ_00146247 -->

    <owl:NamedIndividual rdf:about="http://purl.obolibrary.org/obo/GAZ_00146247">
        <obo:IAO_0000115>A mountain range in the Andes of Peru. Aligned north to south, the main range of some twenty peaks stretches for approximately 25 km, with a subsidiary range of smaller peaks stretching out to the west for approximately 15 km.</obo:IAO_0000115>
        <oboInOwl:hasOBONamespace>GAZ</oboInOwl:hasOBONamespace>
        <oboInOwl:id>GAZ:00146247</oboInOwl:id>
        <rdfs:label>Cordillera Huayhuash</rdfs:label>
    </owl:NamedIndividual>
    


    <!-- http://purl.obolibrary.org/obo/GAZ_00146779 -->

    <owl:NamedIndividual rdf:about="http://purl.obolibrary.org/obo/GAZ_00146779">
        <obo:RO_0001025 rdf:resource="http://purl.obolibrary.org/obo/GAZ_00007836"/>
        <obo:RO_0001025 rdf:resource="http://purl.obolibrary.org/obo/GAZ_22223511"/>
        <obo:IAO_0000115>An island in Lake Maracaibo.</obo:IAO_0000115>
        <oboInOwl:hasOBONamespace>GAZ</oboInOwl:hasOBONamespace>
        <oboInOwl:id>GAZ:00146779</oboInOwl:id>
        <rdfs:label>San Carlos Island</rdfs:label>
    </owl:NamedIndividual>
    


    <!-- http://purl.obolibrary.org/obo/GAZ_00146780 -->

    <owl:NamedIndividual rdf:about="http://purl.obolibrary.org/obo/GAZ_00146780">
        <obo:RO_0001025 rdf:resource="http://purl.obolibrary.org/obo/GAZ_00007836"/>
        <obo:RO_0001025 rdf:resource="http://purl.obolibrary.org/obo/GAZ_22223511"/>
        <obo:IAO_0000115>An island in Lake Maracaibo.</obo:IAO_0000115>
        <oboInOwl:hasOBONamespace>GAZ</oboInOwl:hasOBONamespace>
        <oboInOwl:id>GAZ:00146780</oboInOwl:id>
        <rdfs:label>Los Pajaros Island</rdfs:label>
    </owl:NamedIndividual>
    


    <!-- http://purl.obolibrary.org/obo/GAZ_00146781 -->

    <owl:NamedIndividual rdf:about="http://purl.obolibrary.org/obo/GAZ_00146781">
        <obo:RO_0001025 rdf:resource="http://purl.obolibrary.org/obo/GAZ_00007836"/>
        <obo:RO_0001025 rdf:resource="http://purl.obolibrary.org/obo/GAZ_22223511"/>
        <obo:IAO_0000115>An island in Lake Maracaibo.</obo:IAO_0000115>
        <oboInOwl:hasOBONamespace>GAZ</oboInOwl:hasOBONamespace>
        <oboInOwl:id>GAZ:00146781</oboInOwl:id>
        <rdfs:label>Los Tortuguillos Island</rdfs:label>
    </owl:NamedIndividual>
    


    <!-- http://purl.obolibrary.org/obo/GAZ_00146782 -->

    <owl:NamedIndividual rdf:about="http://purl.obolibrary.org/obo/GAZ_00146782">
        <obo:RO_0001025 rdf:resource="http://purl.obolibrary.org/obo/GAZ_00007836"/>
        <obo:RO_0001025 rdf:resource="http://purl.obolibrary.org/obo/GAZ_22223511"/>
        <obo:IAO_0000115>An island in Lake Maracaibo.</obo:IAO_0000115>
        <oboInOwl:hasOBONamespace>GAZ</oboInOwl:hasOBONamespace>
        <oboInOwl:id>GAZ:00146782</oboInOwl:id>
        <rdfs:label>Toas Island</rdfs:label>
    </owl:NamedIndividual>
    


    <!-- http://purl.obolibrary.org/obo/GAZ_00146783 -->

    <owl:NamedIndividual rdf:about="http://purl.obolibrary.org/obo/GAZ_00146783">
        <obo:RO_0001025 rdf:resource="http://purl.obolibrary.org/obo/GAZ_00007836"/>
        <obo:RO_0001025 rdf:resource="http://purl.obolibrary.org/obo/GAZ_22223511"/>
        <obo:IAO_0000115>An island in Lake Maracaibo.</obo:IAO_0000115>
        <oboInOwl:hasOBONamespace>GAZ</oboInOwl:hasOBONamespace>
        <oboInOwl:id>GAZ:00146783</oboInOwl:id>
        <rdfs:label>Maraca Island</rdfs:label>
    </owl:NamedIndividual>
    


    <!-- http://purl.obolibrary.org/obo/GAZ_00146784 -->

    <owl:NamedIndividual rdf:about="http://purl.obolibrary.org/obo/GAZ_00146784">
        <obo:RO_0001025 rdf:resource="http://purl.obolibrary.org/obo/GAZ_00007836"/>
        <obo:RO_0001025 rdf:resource="http://purl.obolibrary.org/obo/GAZ_22223511"/>
        <obo:IAO_0000115>An island in Lake Maracaibo.</obo:IAO_0000115>
        <oboInOwl:hasOBONamespace>GAZ</oboInOwl:hasOBONamespace>
        <oboInOwl:id>GAZ:00146784</oboInOwl:id>
        <rdfs:label>Zapara Island</rdfs:label>
    </owl:NamedIndividual>
    


    <!-- http://purl.obolibrary.org/obo/GAZ_00146785 -->

    <owl:NamedIndividual rdf:about="http://purl.obolibrary.org/obo/GAZ_00146785">
        <obo:RO_0001025 rdf:resource="http://purl.obolibrary.org/obo/GAZ_00007836"/>
        <obo:RO_0001025 rdf:resource="http://purl.obolibrary.org/obo/GAZ_22223511"/>
        <obo:IAO_0000115>An island in Lake Maracaibo.</obo:IAO_0000115>
        <oboInOwl:hasOBONamespace>GAZ</oboInOwl:hasOBONamespace>
        <oboInOwl:id>GAZ:00146785</oboInOwl:id>
        <rdfs:label>Sabaneta de Montiel Island</rdfs:label>
    </owl:NamedIndividual>
    


    <!-- http://purl.obolibrary.org/obo/GAZ_00146786 -->

    <owl:NamedIndividual rdf:about="http://purl.obolibrary.org/obo/GAZ_00146786">
        <obo:RO_0001025 rdf:resource="http://purl.obolibrary.org/obo/GAZ_00007836"/>
        <obo:RO_0001025 rdf:resource="http://purl.obolibrary.org/obo/GAZ_22223511"/>
        <obo:IAO_0000115>An island in Lake Maracaibo.</obo:IAO_0000115>
        <oboInOwl:hasOBONamespace>GAZ</oboInOwl:hasOBONamespace>
        <oboInOwl:id>GAZ:00146786</oboInOwl:id>
        <rdfs:label>Isla de Providencia</rdfs:label>
    </owl:NamedIndividual>
    


    <!-- http://purl.obolibrary.org/obo/GAZ_00146787 -->

    <owl:NamedIndividual rdf:about="http://purl.obolibrary.org/obo/GAZ_00146787">
        <obo:RO_0001025 rdf:resource="http://purl.obolibrary.org/obo/GAZ_00007836"/>
        <obo:RO_0001025 rdf:resource="http://purl.obolibrary.org/obo/GAZ_22223511"/>
        <obo:IAO_0000115>An island in Lake Maracaibo.</obo:IAO_0000115>
        <oboInOwl:hasOBONamespace>GAZ</oboInOwl:hasOBONamespace>
        <oboInOwl:id>GAZ:00146787</oboInOwl:id>
        <rdfs:label>Isla de Pescadores</rdfs:label>
    </owl:NamedIndividual>
    


    <!-- http://purl.obolibrary.org/obo/GAZ_00146788 -->

    <owl:NamedIndividual rdf:about="http://purl.obolibrary.org/obo/GAZ_00146788">
        <obo:RO_0001025 rdf:resource="http://purl.obolibrary.org/obo/GAZ_00007836"/>
        <obo:RO_0001025 rdf:resource="http://purl.obolibrary.org/obo/GAZ_22223511"/>
        <obo:IAO_0000115>An island in Lake Maracaibo.</obo:IAO_0000115>
        <oboInOwl:hasOBONamespace>GAZ</oboInOwl:hasOBONamespace>
        <oboInOwl:id>GAZ:00146788</oboInOwl:id>
        <rdfs:label>San Bernardo Island</rdfs:label>
    </owl:NamedIndividual>
    


    <!-- http://purl.obolibrary.org/obo/GAZ_00246822 -->

    <owl:NamedIndividual rdf:about="http://purl.obolibrary.org/obo/GAZ_00246822">
        <obo:RO_0001025 rdf:resource="http://purl.obolibrary.org/obo/GAZ_00120718"/>
        <obo:IAO_0000115>A saline lake.</obo:IAO_0000115>
        <oboInOwl:hasOBONamespace>GAZ</oboInOwl:hasOBONamespace>
        <oboInOwl:id>GAZ:00246822</oboInOwl:id>
        <rdfs:label>Salar de Pastos Grandes</rdfs:label>
    </owl:NamedIndividual>
    


    <!-- http://purl.obolibrary.org/obo/GAZ_00246823 -->

    <owl:NamedIndividual rdf:about="http://purl.obolibrary.org/obo/GAZ_00246823">
        <obo:RO_0001025 rdf:resource="http://purl.obolibrary.org/obo/GAZ_00120718"/>
        <obo:IAO_0000115>A saline lake.</obo:IAO_0000115>
        <oboInOwl:hasOBONamespace>GAZ</oboInOwl:hasOBONamespace>
        <oboInOwl:id>GAZ:00246823</oboInOwl:id>
        <rdfs:label>Laguna Hedionda</rdfs:label>
    </owl:NamedIndividual>
    


    <!-- http://purl.obolibrary.org/obo/GAZ_00246824 -->

    <owl:NamedIndividual rdf:about="http://purl.obolibrary.org/obo/GAZ_00246824">
        <obo:RO_0001025 rdf:resource="http://purl.obolibrary.org/obo/GAZ_00120718"/>
        <obo:IAO_0000115>A saline lake.</obo:IAO_0000115>
        <oboInOwl:hasOBONamespace>GAZ</oboInOwl:hasOBONamespace>
        <oboInOwl:id>GAZ:00246824</oboInOwl:id>
        <rdfs:label>Laguna Canapa</rdfs:label>
    </owl:NamedIndividual>
    


    <!-- http://purl.obolibrary.org/obo/GAZ_00246825 -->

    <owl:NamedIndividual rdf:about="http://purl.obolibrary.org/obo/GAZ_00246825">
        <obo:RO_0001025 rdf:resource="http://purl.obolibrary.org/obo/GAZ_00120718"/>
        <obo:IAO_0000115>A saline lake.</obo:IAO_0000115>
        <oboInOwl:hasOBONamespace>GAZ</oboInOwl:hasOBONamespace>
        <oboInOwl:id>GAZ:00246825</oboInOwl:id>
        <rdfs:label>Laguna Ramaditas</rdfs:label>
    </owl:NamedIndividual>
    


    <!-- http://purl.obolibrary.org/obo/GAZ_00246826 -->

    <owl:NamedIndividual rdf:about="http://purl.obolibrary.org/obo/GAZ_00246826">
        <obo:RO_0001025 rdf:resource="http://purl.obolibrary.org/obo/GAZ_00120718"/>
        <obo:IAO_0000115>A saline lake.</obo:IAO_0000115>
        <oboInOwl:hasOBONamespace>GAZ</oboInOwl:hasOBONamespace>
        <oboInOwl:id>GAZ:00246826</oboInOwl:id>
        <rdfs:label>Laguna Cachi</rdfs:label>
    </owl:NamedIndividual>
    


    <!-- http://purl.obolibrary.org/obo/GAZ_00246827 -->

    <owl:NamedIndividual rdf:about="http://purl.obolibrary.org/obo/GAZ_00246827">
        <obo:RO_0001025 rdf:resource="http://purl.obolibrary.org/obo/GAZ_00120718"/>
        <obo:IAO_0000115>A saline lake.</obo:IAO_0000115>
        <oboInOwl:hasOBONamespace>GAZ</oboInOwl:hasOBONamespace>
        <oboInOwl:id>GAZ:00246827</oboInOwl:id>
        <rdfs:label>Laguna Khara</rdfs:label>
    </owl:NamedIndividual>
    


    <!-- http://purl.obolibrary.org/obo/GAZ_00246828 -->

    <owl:NamedIndividual rdf:about="http://purl.obolibrary.org/obo/GAZ_00246828">
        <obo:RO_0001025 rdf:resource="http://purl.obolibrary.org/obo/GAZ_00120718"/>
        <obo:IAO_0000115>A saline lake.</obo:IAO_0000115>
        <oboInOwl:hasOBONamespace>GAZ</oboInOwl:hasOBONamespace>
        <oboInOwl:id>GAZ:00246828</oboInOwl:id>
        <rdfs:label>Laguna Khar Khota</rdfs:label>
    </owl:NamedIndividual>
    


    <!-- http://purl.obolibrary.org/obo/GAZ_00246829 -->

    <owl:NamedIndividual rdf:about="http://purl.obolibrary.org/obo/GAZ_00246829">
        <obo:RO_0001025 rdf:resource="http://purl.obolibrary.org/obo/GAZ_00120718"/>
        <obo:IAO_0000115>A saline lake.</obo:IAO_0000115>
        <oboInOwl:hasOBONamespace>GAZ</oboInOwl:hasOBONamespace>
        <oboInOwl:id>GAZ:00246829</oboInOwl:id>
        <rdfs:label>Laguna Chulluncani</rdfs:label>
    </owl:NamedIndividual>
    


    <!-- http://purl.obolibrary.org/obo/GAZ_00246888 -->

    <owl:NamedIndividual rdf:about="http://purl.obolibrary.org/obo/GAZ_00246888">
        <obo:IAO_0000115>A group of 6 lakes in the highlands of the upper Rio Negro of Brazil.</obo:IAO_0000115>
        <oboInOwl:hasOBONamespace>GAZ</oboInOwl:hasOBONamespace>
        <oboInOwl:id>GAZ:00246888</oboInOwl:id>
        <rdfs:label>Morro de 6 Lagos</rdfs:label>
    </owl:NamedIndividual>
    


    <!-- http://purl.obolibrary.org/obo/GAZ_00246921 -->

    <owl:NamedIndividual rdf:about="http://purl.obolibrary.org/obo/GAZ_00246921">
        <obo:RO_0001025 rdf:resource="http://purl.obolibrary.org/obo/GAZ_00047131"/>
        <obo:IAO_0000115>An island.</obo:IAO_0000115>
        <oboInOwl:hasOBONamespace>GAZ</oboInOwl:hasOBONamespace>
        <oboInOwl:id>GAZ:00246921</oboInOwl:id>
        <rdfs:label>Ilha do Brique</rdfs:label>
    </owl:NamedIndividual>
    


    <!-- http://purl.obolibrary.org/obo/GAZ_00246922 -->

    <owl:NamedIndividual rdf:about="http://purl.obolibrary.org/obo/GAZ_00246922">
        <obo:RO_0001025 rdf:resource="http://purl.obolibrary.org/obo/GAZ_00047131"/>
        <obo:IAO_0000115>An island.</obo:IAO_0000115>
        <oboInOwl:hasOBONamespace>GAZ</oboInOwl:hasOBONamespace>
        <oboInOwl:id>GAZ:00246922</oboInOwl:id>
        <rdfs:label>Ilha Janauco</rdfs:label>
    </owl:NamedIndividual>
    


    <!-- http://purl.obolibrary.org/obo/GAZ_00246923 -->

    <owl:NamedIndividual rdf:about="http://purl.obolibrary.org/obo/GAZ_00246923">
        <obo:RO_0001025 rdf:resource="http://purl.obolibrary.org/obo/GAZ_00047131"/>
        <obo:IAO_0000115>An island.</obo:IAO_0000115>
        <oboInOwl:hasOBONamespace>GAZ</oboInOwl:hasOBONamespace>
        <oboInOwl:id>GAZ:00246923</oboInOwl:id>
        <rdfs:label>Ilha Mexiana</rdfs:label>
    </owl:NamedIndividual>
    


    <!-- http://purl.obolibrary.org/obo/GAZ_00246935 -->

    <owl:NamedIndividual rdf:about="http://purl.obolibrary.org/obo/GAZ_00246935">
        <obo:RO_0001025 rdf:resource="http://purl.obolibrary.org/obo/GAZ_00047131"/>
        <obo:IAO_0000115>A sea bay.</obo:IAO_0000115>
        <oboInOwl:hasOBONamespace>GAZ</oboInOwl:hasOBONamespace>
        <oboInOwl:id>GAZ:00246935</oboInOwl:id>
        <rdfs:label>Baia de Marajo</rdfs:label>
    </owl:NamedIndividual>
    


    <!-- http://purl.obolibrary.org/obo/GAZ_00246936 -->

    <owl:NamedIndividual rdf:about="http://purl.obolibrary.org/obo/GAZ_00246936">
        <obo:RO_0001025 rdf:resource="http://purl.obolibrary.org/obo/GAZ_00047132"/>
        <obo:IAO_0000115>A brackish lake.</obo:IAO_0000115>
        <oboInOwl:hasOBONamespace>GAZ</oboInOwl:hasOBONamespace>
        <oboInOwl:id>GAZ:00246936</oboInOwl:id>
        <rdfs:label>Lago Arari</rdfs:label>
    </owl:NamedIndividual>
    


    <!-- http://purl.obolibrary.org/obo/GAZ_00247222 -->

    <owl:NamedIndividual rdf:about="http://purl.obolibrary.org/obo/GAZ_00247222">
        <obo:RO_0001025 rdf:resource="http://purl.obolibrary.org/obo/GAZ_00056694"/>
        <obo:IAO_0000115>A brackish lake.</obo:IAO_0000115>
        <oboInOwl:hasOBONamespace>GAZ</oboInOwl:hasOBONamespace>
        <oboInOwl:id>GAZ:00247222</oboInOwl:id>
        <rdfs:label>Lago Parinacota</rdfs:label>
    </owl:NamedIndividual>
    


    <!-- http://purl.obolibrary.org/obo/GAZ_00247249 -->

    <owl:NamedIndividual rdf:about="http://purl.obolibrary.org/obo/GAZ_00247249">
        <obo:RO_0001025 rdf:resource="http://purl.obolibrary.org/obo/GAZ_00056538"/>
        <obo:IAO_0000115>A freshwater lake.</obo:IAO_0000115>
        <oboInOwl:hasOBONamespace>GAZ</oboInOwl:hasOBONamespace>
        <oboInOwl:id>GAZ:00247249</oboInOwl:id>
        <rdfs:label>Lago Verde</rdfs:label>
    </owl:NamedIndividual>
    


    <!-- http://purl.obolibrary.org/obo/GAZ_00247250 -->

    <owl:NamedIndividual rdf:about="http://purl.obolibrary.org/obo/GAZ_00247250">
        <obo:RO_0001025 rdf:resource="http://purl.obolibrary.org/obo/GAZ_00056538"/>
        <obo:IAO_0000115>A freshwater lake.</obo:IAO_0000115>
        <oboInOwl:hasOBONamespace>GAZ</oboInOwl:hasOBONamespace>
        <oboInOwl:id>GAZ:00247250</oboInOwl:id>
        <rdfs:label>Lago Captren</rdfs:label>
    </owl:NamedIndividual>
    


    <!-- http://purl.obolibrary.org/obo/GAZ_00247621 -->

    <owl:NamedIndividual rdf:about="http://purl.obolibrary.org/obo/GAZ_00247621">
        <obo:RO_0001025 rdf:resource="http://purl.obolibrary.org/obo/GAZ_00089680"/>
        <obo:IAO_0000115>A bay.</obo:IAO_0000115>
        <oboInOwl:hasOBONamespace>GAZ</oboInOwl:hasOBONamespace>
        <oboInOwl:id>GAZ:00247621</oboInOwl:id>
        <rdfs:label>Bahia Portete</rdfs:label>
    </owl:NamedIndividual>
    


    <!-- http://purl.obolibrary.org/obo/GAZ_00247622 -->

    <owl:NamedIndividual rdf:about="http://purl.obolibrary.org/obo/GAZ_00247622">
        <obo:RO_0001025 rdf:resource="http://purl.obolibrary.org/obo/GAZ_00089668"/>
        <obo:IAO_0000115>Salt pans.</obo:IAO_0000115>
        <oboInOwl:hasOBONamespace>GAZ</oboInOwl:hasOBONamespace>
        <oboInOwl:id>GAZ:00247622</oboInOwl:id>
        <rdfs:label>Salinas de San Juan</rdfs:label>
    </owl:NamedIndividual>
    


    <!-- http://purl.obolibrary.org/obo/GAZ_00247623 -->

    <owl:NamedIndividual rdf:about="http://purl.obolibrary.org/obo/GAZ_00247623">
        <obo:RO_0001025 rdf:resource="http://purl.obolibrary.org/obo/GAZ_00089668"/>
        <obo:IAO_0000115>A coastal wetland.</obo:IAO_0000115>
        <oboInOwl:hasOBONamespace>GAZ</oboInOwl:hasOBONamespace>
        <oboInOwl:id>GAZ:00247623</oboInOwl:id>
        <rdfs:label>Cienaga de San Angustin</rdfs:label>
    </owl:NamedIndividual>
    


    <!-- http://purl.obolibrary.org/obo/GAZ_00247657 -->

    <owl:NamedIndividual rdf:about="http://purl.obolibrary.org/obo/GAZ_00247657">
        <obo:RO_0001025 rdf:resource="http://purl.obolibrary.org/obo/GAZ_00089702"/>
        <obo:IAO_0000115>A freshwater lake. Located 30 km E of Popayan at the source of the Rio Cauca and Rio Magdalena.</obo:IAO_0000115>
        <oboInOwl:hasOBONamespace>GAZ</oboInOwl:hasOBONamespace>
        <oboInOwl:id>GAZ:00247657</oboInOwl:id>
        <rdfs:label>Laguna San Rafael</rdfs:label>
    </owl:NamedIndividual>
    


    <!-- http://purl.obolibrary.org/obo/GAZ_00247877 -->

    <owl:NamedIndividual rdf:about="http://purl.obolibrary.org/obo/GAZ_00247877">
        <obo:RO_0001025 rdf:resource="http://purl.obolibrary.org/obo/GAZ_00056295"/>
        <obo:IAO_0000115>A freshwater lake occupying a glacial fjord on the NE slopes of Volcan Cayamber.</obo:IAO_0000115>
        <oboInOwl:hasOBONamespace>GAZ</oboInOwl:hasOBONamespace>
        <oboInOwl:id>GAZ:00247877</oboInOwl:id>
        <rdfs:label>Laguna de San Marcos</rdfs:label>
    </owl:NamedIndividual>
    


    <!-- http://purl.obolibrary.org/obo/GAZ_00247879 -->

    <owl:NamedIndividual rdf:about="http://purl.obolibrary.org/obo/GAZ_00247879">
        <obo:RO_0001025 rdf:resource="http://purl.obolibrary.org/obo/GAZ_00056292"/>
        <obo:IAO_0000115>A freshwater lake on the S slope of Volcan Antisana.</obo:IAO_0000115>
        <oboInOwl:hasOBONamespace>GAZ</oboInOwl:hasOBONamespace>
        <oboInOwl:id>GAZ:00247879</oboInOwl:id>
        <rdfs:label>Lago La Mica</rdfs:label>
    </owl:NamedIndividual>
    


    <!-- http://purl.obolibrary.org/obo/GAZ_00247880 -->

    <owl:NamedIndividual rdf:about="http://purl.obolibrary.org/obo/GAZ_00247880">
        <obo:RO_0001025 rdf:resource="http://purl.obolibrary.org/obo/GAZ_00056298"/>
        <obo:IAO_0000115>A freshwater lake below the peak of Volcan Cotopaxi.</obo:IAO_0000115>
        <oboInOwl:hasOBONamespace>GAZ</oboInOwl:hasOBONamespace>
        <oboInOwl:id>GAZ:00247880</oboInOwl:id>
        <rdfs:label>Limpiapungo Lake</rdfs:label>
    </owl:NamedIndividual>
    


    <!-- http://purl.obolibrary.org/obo/GAZ_00247882 -->

    <owl:NamedIndividual rdf:about="http://purl.obolibrary.org/obo/GAZ_00247882">
        <obo:RO_0001025 rdf:resource="http://purl.obolibrary.org/obo/GAZ_00247884"/>
        <obo:IAO_0000115>A glacial lake on Cerro Yanaurco.</obo:IAO_0000115>
        <oboInOwl:hasOBONamespace>GAZ</oboInOwl:hasOBONamespace>
        <oboInOwl:id>GAZ:00247882</oboInOwl:id>
        <rdfs:label>Laguna de Kingora</rdfs:label>
    </owl:NamedIndividual>
    


    <!-- http://purl.obolibrary.org/obo/GAZ_00247883 -->

    <owl:NamedIndividual rdf:about="http://purl.obolibrary.org/obo/GAZ_00247883">
        <obo:RO_0001025 rdf:resource="http://purl.obolibrary.org/obo/GAZ_00247884"/>
        <obo:IAO_0000115>A glacial lake on Cerro Yanaurco.</obo:IAO_0000115>
        <oboInOwl:hasOBONamespace>GAZ</oboInOwl:hasOBONamespace>
        <oboInOwl:id>GAZ:00247883</oboInOwl:id>
        <rdfs:label>Lago de Culebrillas</rdfs:label>
    </owl:NamedIndividual>
    


    <!-- http://purl.obolibrary.org/obo/GAZ_00247884 -->

    <owl:NamedIndividual rdf:about="http://purl.obolibrary.org/obo/GAZ_00247884">
        <obo:IAO_0000115>A mountain.</obo:IAO_0000115>
        <oboInOwl:hasOBONamespace>GAZ</oboInOwl:hasOBONamespace>
        <oboInOwl:id>GAZ:00247884</oboInOwl:id>
        <rdfs:label>Cerro Yanaurco</rdfs:label>
    </owl:NamedIndividual>
    


    <!-- http://purl.obolibrary.org/obo/GAZ_00254087 -->

    <owl:NamedIndividual rdf:about="http://purl.obolibrary.org/obo/GAZ_00254087">
        <obo:RO_0001025 rdf:resource="http://purl.obolibrary.org/obo/GAZ_00047130"/>
        <obo:IAO_0000115>A river that rises north of Lake Titicaca, in the Arequipa region of South America.</obo:IAO_0000115>
        <oboInOwl:hasOBONamespace>GAZ</oboInOwl:hasOBONamespace>
        <oboInOwl:id>GAZ:00254087</oboInOwl:id>
        <rdfs:label>Rio Ucayali</rdfs:label>
    </owl:NamedIndividual>
    


    <!-- http://purl.obolibrary.org/obo/GAZ_00260060 -->

    <owl:NamedIndividual rdf:about="http://purl.obolibrary.org/obo/GAZ_00260060">
        <obo:RO_0001025 rdf:resource="http://purl.obolibrary.org/obo/GAZ_00011626"/>
        <obo:IAO_0000115>An asphalt lake.</obo:IAO_0000115>
        <oboInOwl:hasOBONamespace>GAZ</oboInOwl:hasOBONamespace>
        <oboInOwl:id>GAZ:00260060</oboInOwl:id>
        <rdfs:label>Lago Guanico</rdfs:label>
    </owl:NamedIndividual>
    


    <!-- http://purl.obolibrary.org/obo/GAZ_02000849 -->

    <owl:NamedIndividual rdf:about="http://purl.obolibrary.org/obo/GAZ_02000849">
        <obo:RO_0001025 rdf:resource="http://purl.obolibrary.org/obo/GAZ_00005073"/>
    </owl:NamedIndividual>
    


    <!-- http://purl.obolibrary.org/obo/GAZ_04000006 -->

    <owl:NamedIndividual rdf:about="http://purl.obolibrary.org/obo/GAZ_04000006">
        <obo:RO_0001025 rdf:resource="http://purl.obolibrary.org/obo/GAZ_00011584"/>
        <oboInOwl:hasOBONamespace>GAZ</oboInOwl:hasOBONamespace>
        <oboInOwl:id>GAZ:04000006</oboInOwl:id>
        <rdfs:label>Municipality of Achaguas</rdfs:label>
    </owl:NamedIndividual>
    


    <!-- http://purl.obolibrary.org/obo/GAZ_04000007 -->

    <owl:NamedIndividual rdf:about="http://purl.obolibrary.org/obo/GAZ_04000007">
        <obo:RO_0001025 rdf:resource="http://purl.obolibrary.org/obo/GAZ_00011584"/>
        <oboInOwl:hasOBONamespace>GAZ</oboInOwl:hasOBONamespace>
        <oboInOwl:id>GAZ:04000007</oboInOwl:id>
        <rdfs:label>Municipality of San Fernando</rdfs:label>
    </owl:NamedIndividual>
    


    <!-- http://purl.obolibrary.org/obo/GAZ_04000008 -->

    <owl:NamedIndividual rdf:about="http://purl.obolibrary.org/obo/GAZ_04000008">
        <obo:RO_0001025 rdf:resource="http://purl.obolibrary.org/obo/GAZ_00011588"/>
        <oboInOwl:hasOBONamespace>GAZ</oboInOwl:hasOBONamespace>
        <oboInOwl:id>GAZ:04000008</oboInOwl:id>
        <rdfs:label>Municipality of Arismendi</rdfs:label>
    </owl:NamedIndividual>
    


    <!-- http://purl.obolibrary.org/obo/GAZ_04000009 -->

    <owl:NamedIndividual rdf:about="http://purl.obolibrary.org/obo/GAZ_04000009">
        <obo:RO_0001025 rdf:resource="http://purl.obolibrary.org/obo/GAZ_00011592"/>
        <oboInOwl:hasOBONamespace>GAZ</oboInOwl:hasOBONamespace>
        <oboInOwl:id>GAZ:04000009</oboInOwl:id>
        <rdfs:label>Municipality of Anzoategui</rdfs:label>
    </owl:NamedIndividual>
    


    <!-- http://purl.obolibrary.org/obo/GAZ_04000010 -->

    <owl:NamedIndividual rdf:about="http://purl.obolibrary.org/obo/GAZ_04000010">
        <obo:RO_0001025 rdf:resource="http://purl.obolibrary.org/obo/GAZ_00011598"/>
        <oboInOwl:hasOBONamespace>GAZ</oboInOwl:hasOBONamespace>
        <oboInOwl:id>GAZ:04000010</oboInOwl:id>
        <rdfs:label>Municipality of Guanare</rdfs:label>
    </owl:NamedIndividual>
    


    <!-- http://purl.obolibrary.org/obo/GAZ_04000011 -->

    <owl:NamedIndividual rdf:about="http://purl.obolibrary.org/obo/GAZ_04000011">
        <obo:RO_0001025 rdf:resource="http://purl.obolibrary.org/obo/GAZ_00011598"/>
        <oboInOwl:hasOBONamespace>GAZ</oboInOwl:hasOBONamespace>
        <oboInOwl:id>GAZ:04000011</oboInOwl:id>
        <rdfs:label>Municipality of Esteller</rdfs:label>
    </owl:NamedIndividual>
    


    <!-- http://purl.obolibrary.org/obo/GAZ_22223392 -->

    <owl:NamedIndividual rdf:about="http://purl.obolibrary.org/obo/GAZ_22223392">
        <obo:RO_0001025 rdf:resource="http://purl.obolibrary.org/obo/GAZ_00011592"/>
        <oboInOwl:hasOBONamespace>GAZ</oboInOwl:hasOBONamespace>
        <oboInOwl:id>GAZ:22223392</oboInOwl:id>
        <rdfs:label>Municipality of El Pao de San Juan Bautista</rdfs:label>
    </owl:NamedIndividual>
    


    <!-- http://purl.obolibrary.org/obo/GAZ_22223393 -->

    <owl:NamedIndividual rdf:about="http://purl.obolibrary.org/obo/GAZ_22223393">
        <obo:RO_0001025 rdf:resource="http://purl.obolibrary.org/obo/GAZ_00011592"/>
        <oboInOwl:hasOBONamespace>GAZ</oboInOwl:hasOBONamespace>
        <oboInOwl:id>GAZ:22223393</oboInOwl:id>
        <rdfs:label>Municipality of Falcon</rdfs:label>
    </owl:NamedIndividual>
    


    <!-- http://purl.obolibrary.org/obo/GAZ_22223394 -->

    <owl:NamedIndividual rdf:about="http://purl.obolibrary.org/obo/GAZ_22223394">
        <obo:RO_0001025 rdf:resource="http://purl.obolibrary.org/obo/GAZ_00011592"/>
        <oboInOwl:hasOBONamespace>GAZ</oboInOwl:hasOBONamespace>
        <oboInOwl:id>GAZ:22223394</oboInOwl:id>
        <rdfs:label>Municipality of Girardot</rdfs:label>
    </owl:NamedIndividual>
    


    <!-- http://purl.obolibrary.org/obo/GAZ_22223395 -->

    <owl:NamedIndividual rdf:about="http://purl.obolibrary.org/obo/GAZ_22223395">
        <obo:RO_0001025 rdf:resource="http://purl.obolibrary.org/obo/GAZ_00011592"/>
        <oboInOwl:hasOBONamespace>GAZ</oboInOwl:hasOBONamespace>
        <oboInOwl:id>GAZ:22223395</oboInOwl:id>
        <rdfs:label>Municipality of Lima Blanco</rdfs:label>
    </owl:NamedIndividual>
    


    <!-- http://purl.obolibrary.org/obo/GAZ_22223396 -->

    <owl:NamedIndividual rdf:about="http://purl.obolibrary.org/obo/GAZ_22223396">
        <obo:RO_0001025 rdf:resource="http://purl.obolibrary.org/obo/GAZ_00011592"/>
        <oboInOwl:hasOBONamespace>GAZ</oboInOwl:hasOBONamespace>
        <oboInOwl:id>GAZ:22223396</oboInOwl:id>
        <rdfs:label>Municipality of Ricaurte</rdfs:label>
    </owl:NamedIndividual>
    


    <!-- http://purl.obolibrary.org/obo/GAZ_22223397 -->

    <owl:NamedIndividual rdf:about="http://purl.obolibrary.org/obo/GAZ_22223397">
        <obo:RO_0001025 rdf:resource="http://purl.obolibrary.org/obo/GAZ_00011592"/>
        <oboInOwl:hasOBONamespace>GAZ</oboInOwl:hasOBONamespace>
        <oboInOwl:id>GAZ:22223397</oboInOwl:id>
        <rdfs:label>Municipality of Romulo Gallegos</rdfs:label>
    </owl:NamedIndividual>
    


    <!-- http://purl.obolibrary.org/obo/GAZ_22223398 -->

    <owl:NamedIndividual rdf:about="http://purl.obolibrary.org/obo/GAZ_22223398">
        <obo:RO_0001025 rdf:resource="http://purl.obolibrary.org/obo/GAZ_00011592"/>
        <oboInOwl:hasOBONamespace>GAZ</oboInOwl:hasOBONamespace>
        <oboInOwl:id>GAZ:22223398</oboInOwl:id>
        <rdfs:label>Municipality of San Carlos de Austria</rdfs:label>
    </owl:NamedIndividual>
    


    <!-- http://purl.obolibrary.org/obo/GAZ_22223399 -->

    <owl:NamedIndividual rdf:about="http://purl.obolibrary.org/obo/GAZ_22223399">
        <obo:RO_0001025 rdf:resource="http://purl.obolibrary.org/obo/GAZ_00011592"/>
        <oboInOwl:hasOBONamespace>GAZ</oboInOwl:hasOBONamespace>
        <oboInOwl:id>GAZ:22223399</oboInOwl:id>
        <rdfs:label>Municipality of Tinaco</rdfs:label>
    </owl:NamedIndividual>
    


    <!-- http://purl.obolibrary.org/obo/GAZ_22223400 -->

    <owl:NamedIndividual rdf:about="http://purl.obolibrary.org/obo/GAZ_22223400">
        <obo:RO_0001025 rdf:resource="http://purl.obolibrary.org/obo/GAZ_22223398"/>
        <oboInOwl:hasOBONamespace>GAZ</oboInOwl:hasOBONamespace>
        <oboInOwl:id>GAZ:22223400</oboInOwl:id>
        <rdfs:label>Cano Hondo</rdfs:label>
    </owl:NamedIndividual>
    


    <!-- http://purl.obolibrary.org/obo/GAZ_22223401 -->

    <owl:NamedIndividual rdf:about="http://purl.obolibrary.org/obo/GAZ_22223401">
        <obo:RO_0001025 rdf:resource="http://purl.obolibrary.org/obo/GAZ_00011584"/>
        <oboInOwl:hasOBONamespace>GAZ</oboInOwl:hasOBONamespace>
        <oboInOwl:id>GAZ:22223401</oboInOwl:id>
        <rdfs:label>Municipality of Biruaca</rdfs:label>
    </owl:NamedIndividual>
    


    <!-- http://purl.obolibrary.org/obo/GAZ_22223402 -->

    <owl:NamedIndividual rdf:about="http://purl.obolibrary.org/obo/GAZ_22223402">
        <obo:RO_0001025 rdf:resource="http://purl.obolibrary.org/obo/GAZ_00011584"/>
        <oboInOwl:hasOBONamespace>GAZ</oboInOwl:hasOBONamespace>
        <oboInOwl:id>GAZ:22223402</oboInOwl:id>
        <rdfs:label>Municipality of Pedro Camejo</rdfs:label>
    </owl:NamedIndividual>
    


    <!-- http://purl.obolibrary.org/obo/GAZ_22223403 -->

    <owl:NamedIndividual rdf:about="http://purl.obolibrary.org/obo/GAZ_22223403">
        <obo:RO_0001025 rdf:resource="http://purl.obolibrary.org/obo/GAZ_00011584"/>
        <oboInOwl:hasOBONamespace>GAZ</oboInOwl:hasOBONamespace>
        <oboInOwl:id>GAZ:22223403</oboInOwl:id>
        <rdfs:label>Municipality of Paez</rdfs:label>
    </owl:NamedIndividual>
    


    <!-- http://purl.obolibrary.org/obo/GAZ_22223404 -->

    <owl:NamedIndividual rdf:about="http://purl.obolibrary.org/obo/GAZ_22223404">
        <obo:RO_0001025 rdf:resource="http://purl.obolibrary.org/obo/GAZ_00011584"/>
        <oboInOwl:hasOBONamespace>GAZ</oboInOwl:hasOBONamespace>
        <oboInOwl:id>GAZ:22223404</oboInOwl:id>
        <rdfs:label>Municipality of Munoz</rdfs:label>
    </owl:NamedIndividual>
    


    <!-- http://purl.obolibrary.org/obo/GAZ_22223405 -->

    <owl:NamedIndividual rdf:about="http://purl.obolibrary.org/obo/GAZ_22223405">
        <obo:RO_0001025 rdf:resource="http://purl.obolibrary.org/obo/GAZ_00011584"/>
        <oboInOwl:hasOBONamespace>GAZ</oboInOwl:hasOBONamespace>
        <oboInOwl:id>GAZ:22223405</oboInOwl:id>
        <rdfs:label>Municipality of Romulo Gallegos</rdfs:label>
    </owl:NamedIndividual>
    


    <!-- http://purl.obolibrary.org/obo/GAZ_22223489 -->

    <owl:NamedIndividual rdf:about="http://purl.obolibrary.org/obo/GAZ_22223489">
        <obo:RO_0001025 rdf:resource="http://purl.obolibrary.org/obo/GAZ_00009151"/>
        <oboInOwl:hasOBONamespace>GAZ</oboInOwl:hasOBONamespace>
        <oboInOwl:id>GAZ:22223489</oboInOwl:id>
        <rdfs:label>Municipality of Anaco</rdfs:label>
    </owl:NamedIndividual>
    


    <!-- http://purl.obolibrary.org/obo/GAZ_22223490 -->

    <owl:NamedIndividual rdf:about="http://purl.obolibrary.org/obo/GAZ_22223490">
        <obo:RO_0001025 rdf:resource="http://purl.obolibrary.org/obo/GAZ_00009151"/>
        <oboInOwl:hasOBONamespace>GAZ</oboInOwl:hasOBONamespace>
        <oboInOwl:id>GAZ:22223490</oboInOwl:id>
        <rdfs:label>Municipality of Diego Bautista Urbaneja</rdfs:label>
    </owl:NamedIndividual>
    


    <!-- http://purl.obolibrary.org/obo/GAZ_22223491 -->

    <owl:NamedIndividual rdf:about="http://purl.obolibrary.org/obo/GAZ_22223491">
        <obo:RO_0001025 rdf:resource="http://purl.obolibrary.org/obo/GAZ_00009151"/>
        <oboInOwl:hasOBONamespace>GAZ</oboInOwl:hasOBONamespace>
        <oboInOwl:id>GAZ:22223491</oboInOwl:id>
        <rdfs:label>Municipality of Aragua</rdfs:label>
    </owl:NamedIndividual>
    


    <!-- http://purl.obolibrary.org/obo/GAZ_22223492 -->

    <owl:NamedIndividual rdf:about="http://purl.obolibrary.org/obo/GAZ_22223492">
        <obo:RO_0001025 rdf:resource="http://purl.obolibrary.org/obo/GAZ_00009151"/>
        <oboInOwl:hasOBONamespace>GAZ</oboInOwl:hasOBONamespace>
        <oboInOwl:id>GAZ:22223492</oboInOwl:id>
        <rdfs:label>Municipality of Francisco de Carmen Carvajal</rdfs:label>
    </owl:NamedIndividual>
    


    <!-- http://purl.obolibrary.org/obo/GAZ_22223493 -->

    <owl:NamedIndividual rdf:about="http://purl.obolibrary.org/obo/GAZ_22223493">
        <obo:RO_0001025 rdf:resource="http://purl.obolibrary.org/obo/GAZ_00009151"/>
        <oboInOwl:hasOBONamespace>GAZ</oboInOwl:hasOBONamespace>
        <oboInOwl:id>GAZ:22223493</oboInOwl:id>
        <rdfs:label>Municipality of Fernando de Penalver</rdfs:label>
    </owl:NamedIndividual>
    


    <!-- http://purl.obolibrary.org/obo/GAZ_22223494 -->

    <owl:NamedIndividual rdf:about="http://purl.obolibrary.org/obo/GAZ_22223494">
        <obo:RO_0001025 rdf:resource="http://purl.obolibrary.org/obo/GAZ_00009151"/>
        <oboInOwl:hasOBONamespace>GAZ</oboInOwl:hasOBONamespace>
        <oboInOwl:id>GAZ:22223494</oboInOwl:id>
        <rdfs:label>Municipality of Independencia</rdfs:label>
    </owl:NamedIndividual>
    


    <!-- http://purl.obolibrary.org/obo/GAZ_22223495 -->

    <owl:NamedIndividual rdf:about="http://purl.obolibrary.org/obo/GAZ_22223495">
        <obo:RO_0001025 rdf:resource="http://purl.obolibrary.org/obo/GAZ_00009151"/>
        <oboInOwl:hasOBONamespace>GAZ</oboInOwl:hasOBONamespace>
        <oboInOwl:id>GAZ:22223495</oboInOwl:id>
        <rdfs:label>Municipality of Francisco de Miranda</rdfs:label>
    </owl:NamedIndividual>
    


    <!-- http://purl.obolibrary.org/obo/GAZ_22223496 -->

    <owl:NamedIndividual rdf:about="http://purl.obolibrary.org/obo/GAZ_22223496">
        <obo:RO_0001025 rdf:resource="http://purl.obolibrary.org/obo/GAZ_00009151"/>
        <oboInOwl:hasOBONamespace>GAZ</oboInOwl:hasOBONamespace>
        <oboInOwl:id>GAZ:22223496</oboInOwl:id>
        <rdfs:label>Municipality of Juan Antonio Sotillo</rdfs:label>
    </owl:NamedIndividual>
    


    <!-- http://purl.obolibrary.org/obo/GAZ_22223497 -->

    <owl:NamedIndividual rdf:about="http://purl.obolibrary.org/obo/GAZ_22223497">
        <obo:RO_0001025 rdf:resource="http://purl.obolibrary.org/obo/GAZ_00009151"/>
        <oboInOwl:hasOBONamespace>GAZ</oboInOwl:hasOBONamespace>
        <oboInOwl:id>GAZ:22223497</oboInOwl:id>
        <rdfs:label>Municipality of Libertad</rdfs:label>
    </owl:NamedIndividual>
    


    <!-- http://purl.obolibrary.org/obo/GAZ_22223498 -->

    <owl:NamedIndividual rdf:about="http://purl.obolibrary.org/obo/GAZ_22223498">
        <obo:RO_0001025 rdf:resource="http://purl.obolibrary.org/obo/GAZ_00009151"/>
        <oboInOwl:hasOBONamespace>GAZ</oboInOwl:hasOBONamespace>
        <oboInOwl:id>GAZ:22223498</oboInOwl:id>
        <rdfs:label>Municipality of Juan Manuel Cajigal</rdfs:label>
    </owl:NamedIndividual>
    


    <!-- http://purl.obolibrary.org/obo/GAZ_22223499 -->

    <owl:NamedIndividual rdf:about="http://purl.obolibrary.org/obo/GAZ_22223499">
        <obo:RO_0001025 rdf:resource="http://purl.obolibrary.org/obo/GAZ_00009151"/>
        <oboInOwl:hasOBONamespace>GAZ</oboInOwl:hasOBONamespace>
        <oboInOwl:id>GAZ:22223499</oboInOwl:id>
        <rdfs:label>Municipality of Jose Gregorio Monagas</rdfs:label>
    </owl:NamedIndividual>
    


    <!-- http://purl.obolibrary.org/obo/GAZ_22223500 -->

    <owl:NamedIndividual rdf:about="http://purl.obolibrary.org/obo/GAZ_22223500">
        <obo:RO_0001025 rdf:resource="http://purl.obolibrary.org/obo/GAZ_00009151"/>
        <oboInOwl:hasOBONamespace>GAZ</oboInOwl:hasOBONamespace>
        <oboInOwl:id>GAZ:22223500</oboInOwl:id>
        <rdfs:label>Municipality of San Jose de Guanipa</rdfs:label>
    </owl:NamedIndividual>
    


    <!-- http://purl.obolibrary.org/obo/GAZ_22223501 -->

    <owl:NamedIndividual rdf:about="http://purl.obolibrary.org/obo/GAZ_22223501">
        <obo:RO_0001025 rdf:resource="http://purl.obolibrary.org/obo/GAZ_00009151"/>
        <oboInOwl:hasOBONamespace>GAZ</oboInOwl:hasOBONamespace>
        <oboInOwl:id>GAZ:22223501</oboInOwl:id>
        <rdfs:label>Municipality of Pedro Maria Freites</rdfs:label>
    </owl:NamedIndividual>
    


    <!-- http://purl.obolibrary.org/obo/GAZ_22223502 -->

    <owl:NamedIndividual rdf:about="http://purl.obolibrary.org/obo/GAZ_22223502">
        <obo:RO_0001025 rdf:resource="http://purl.obolibrary.org/obo/GAZ_00009151"/>
        <oboInOwl:hasOBONamespace>GAZ</oboInOwl:hasOBONamespace>
        <oboInOwl:id>GAZ:22223502</oboInOwl:id>
        <rdfs:label>Municipality of Sir Arthur McGregor</rdfs:label>
    </owl:NamedIndividual>
    


    <!-- http://purl.obolibrary.org/obo/GAZ_22223503 -->

    <owl:NamedIndividual rdf:about="http://purl.obolibrary.org/obo/GAZ_22223503">
        <obo:RO_0001025 rdf:resource="http://purl.obolibrary.org/obo/GAZ_00009151"/>
        <oboInOwl:hasOBONamespace>GAZ</oboInOwl:hasOBONamespace>
        <oboInOwl:id>GAZ:22223503</oboInOwl:id>
        <rdfs:label>Municipality of Manuel Ezequiel Bruzual</rdfs:label>
    </owl:NamedIndividual>
    


    <!-- http://purl.obolibrary.org/obo/GAZ_22223504 -->

    <owl:NamedIndividual rdf:about="http://purl.obolibrary.org/obo/GAZ_22223504">
        <obo:RO_0001025 rdf:resource="http://purl.obolibrary.org/obo/GAZ_00009151"/>
        <oboInOwl:hasOBONamespace>GAZ</oboInOwl:hasOBONamespace>
        <oboInOwl:id>GAZ:22223504</oboInOwl:id>
        <rdfs:label>Municipality of Simon Rodriguez</rdfs:label>
    </owl:NamedIndividual>
    


    <!-- http://purl.obolibrary.org/obo/GAZ_22223505 -->

    <owl:NamedIndividual rdf:about="http://purl.obolibrary.org/obo/GAZ_22223505">
        <obo:RO_0001025 rdf:resource="http://purl.obolibrary.org/obo/GAZ_00009151"/>
        <oboInOwl:hasOBONamespace>GAZ</oboInOwl:hasOBONamespace>
        <oboInOwl:id>GAZ:22223505</oboInOwl:id>
        <rdfs:label>Municipality of Santa Ana</rdfs:label>
    </owl:NamedIndividual>
    


    <!-- http://purl.obolibrary.org/obo/GAZ_22223506 -->

    <owl:NamedIndividual rdf:about="http://purl.obolibrary.org/obo/GAZ_22223506">
        <obo:RO_0001025 rdf:resource="http://purl.obolibrary.org/obo/GAZ_00009151"/>
        <oboInOwl:hasOBONamespace>GAZ</oboInOwl:hasOBONamespace>
        <oboInOwl:id>GAZ:22223506</oboInOwl:id>
        <rdfs:label>Municipality of San Juan de Capistrano</rdfs:label>
    </owl:NamedIndividual>
    


    <!-- http://purl.obolibrary.org/obo/GAZ_22223507 -->

    <owl:NamedIndividual rdf:about="http://purl.obolibrary.org/obo/GAZ_22223507">
        <obo:RO_0001025 rdf:resource="http://purl.obolibrary.org/obo/GAZ_00009151"/>
        <oboInOwl:hasOBONamespace>GAZ</oboInOwl:hasOBONamespace>
        <oboInOwl:id>GAZ:22223507</oboInOwl:id>
        <rdfs:label>Municipality of Simon Bolivar</rdfs:label>
    </owl:NamedIndividual>
    


    <!-- http://purl.obolibrary.org/obo/GAZ_22223508 -->

    <owl:NamedIndividual rdf:about="http://purl.obolibrary.org/obo/GAZ_22223508">
        <obo:RO_0001025 rdf:resource="http://purl.obolibrary.org/obo/GAZ_00009151"/>
        <oboInOwl:hasOBONamespace>GAZ</oboInOwl:hasOBONamespace>
        <oboInOwl:id>GAZ:22223508</oboInOwl:id>
        <rdfs:label>Municipality of Piritu</rdfs:label>
    </owl:NamedIndividual>
    


    <!-- http://purl.obolibrary.org/obo/GAZ_22223509 -->

    <owl:NamedIndividual rdf:about="http://purl.obolibrary.org/obo/GAZ_22223509">
        <obo:RO_0001025 rdf:resource="http://purl.obolibrary.org/obo/GAZ_00011612"/>
        <obo:IAO_0000115>A peninsula in northern Colombia and northwestern Venezuela in the Caribbean sea. It is the northernmost peninsula in South America and has an area of 25,000 km2 extending from the Manaure Bay (Colombia) in the Caribbean sea to the Calabazo Ensenada in the Gulf of Venezuela (Venezuela). Most of the territory is part of Colombia, making part of the Department of La Guajira, while the remaining strip pertains to the Venezuelan State of Zulia. The northern most part of the peninsula is called Punta Gallinas.</obo:IAO_0000115>
        <oboInOwl:hasOBONamespace>GAZ</oboInOwl:hasOBONamespace>
        <oboInOwl:id>GAZ:22223509</oboInOwl:id>
        <rdfs:label>Guajira Peninsula</rdfs:label>
    </owl:NamedIndividual>
    


    <!-- http://purl.obolibrary.org/obo/GAZ_22223510 -->

    <owl:NamedIndividual rdf:about="http://purl.obolibrary.org/obo/GAZ_22223510">
        <obo:RO_0001025 rdf:resource="http://purl.obolibrary.org/obo/GAZ_00011612"/>
        <oboInOwl:hasOBONamespace>GAZ</oboInOwl:hasOBONamespace>
        <oboInOwl:id>GAZ:22223510</oboInOwl:id>
        <rdfs:label>Municipality of Rosario de Perija</rdfs:label>
    </owl:NamedIndividual>
    


    <!-- http://purl.obolibrary.org/obo/GAZ_22223511 -->

    <owl:NamedIndividual rdf:about="http://purl.obolibrary.org/obo/GAZ_22223511">
        <obo:RO_0001025 rdf:resource="http://purl.obolibrary.org/obo/GAZ_00011612"/>
        <oboInOwl:hasOBONamespace>GAZ</oboInOwl:hasOBONamespace>
        <oboInOwl:id>GAZ:22223511</oboInOwl:id>
        <rdfs:label>Municipality of Almirante Padilla</rdfs:label>
    </owl:NamedIndividual>
    


    <!-- http://purl.obolibrary.org/obo/GAZ_22223512 -->

    <owl:NamedIndividual rdf:about="http://purl.obolibrary.org/obo/GAZ_22223512">
        <obo:RO_0001025 rdf:resource="http://purl.obolibrary.org/obo/GAZ_00011612"/>
        <oboInOwl:hasOBONamespace>GAZ</oboInOwl:hasOBONamespace>
        <oboInOwl:id>GAZ:22223512</oboInOwl:id>
        <rdfs:label>Municipality of Cabimas</rdfs:label>
    </owl:NamedIndividual>
    


    <!-- http://purl.obolibrary.org/obo/GAZ_22223513 -->

    <owl:NamedIndividual rdf:about="http://purl.obolibrary.org/obo/GAZ_22223513">
        <obo:RO_0001025 rdf:resource="http://purl.obolibrary.org/obo/GAZ_00011612"/>
        <oboInOwl:hasOBONamespace>GAZ</oboInOwl:hasOBONamespace>
        <oboInOwl:id>GAZ:22223513</oboInOwl:id>
        <rdfs:label>Municipality of Baralt</rdfs:label>
    </owl:NamedIndividual>
    


    <!-- http://purl.obolibrary.org/obo/GAZ_22223514 -->

    <owl:NamedIndividual rdf:about="http://purl.obolibrary.org/obo/GAZ_22223514">
        <obo:RO_0001025 rdf:resource="http://purl.obolibrary.org/obo/GAZ_00011612"/>
        <oboInOwl:hasOBONamespace>GAZ</oboInOwl:hasOBONamespace>
        <oboInOwl:id>GAZ:22223514</oboInOwl:id>
        <rdfs:label>Municipality of Valmore Rodriguez</rdfs:label>
    </owl:NamedIndividual>
    


    <!-- http://purl.obolibrary.org/obo/GAZ_22223515 -->

    <owl:NamedIndividual rdf:about="http://purl.obolibrary.org/obo/GAZ_22223515">
        <obo:RO_0001025 rdf:resource="http://purl.obolibrary.org/obo/GAZ_00011612"/>
        <oboInOwl:hasOBONamespace>GAZ</oboInOwl:hasOBONamespace>
        <oboInOwl:id>GAZ:22223515</oboInOwl:id>
        <rdfs:label>Municipality of Simon Bolivar</rdfs:label>
    </owl:NamedIndividual>
    


    <!-- http://purl.obolibrary.org/obo/GAZ_22223516 -->

    <owl:NamedIndividual rdf:about="http://purl.obolibrary.org/obo/GAZ_22223516">
        <obo:RO_0001025 rdf:resource="http://purl.obolibrary.org/obo/GAZ_00011612"/>
        <oboInOwl:hasOBONamespace>GAZ</oboInOwl:hasOBONamespace>
        <oboInOwl:id>GAZ:22223516</oboInOwl:id>
        <rdfs:label>Municipality of Catatumbo</rdfs:label>
    </owl:NamedIndividual>
    


    <!-- http://purl.obolibrary.org/obo/GAZ_22223517 -->

    <owl:NamedIndividual rdf:about="http://purl.obolibrary.org/obo/GAZ_22223517">
        <obo:RO_0001025 rdf:resource="http://purl.obolibrary.org/obo/GAZ_00011612"/>
        <oboInOwl:hasOBONamespace>GAZ</oboInOwl:hasOBONamespace>
        <oboInOwl:id>GAZ:22223517</oboInOwl:id>
        <rdfs:label>Municipality of Colon</rdfs:label>
    </owl:NamedIndividual>
    


    <!-- http://purl.obolibrary.org/obo/GAZ_22223518 -->

    <owl:NamedIndividual rdf:about="http://purl.obolibrary.org/obo/GAZ_22223518">
        <obo:RO_0001025 rdf:resource="http://purl.obolibrary.org/obo/GAZ_00011612"/>
        <oboInOwl:hasOBONamespace>GAZ</oboInOwl:hasOBONamespace>
        <oboInOwl:id>GAZ:22223518</oboInOwl:id>
        <rdfs:label>Municipality of Jesus Enrique Lossada</rdfs:label>
    </owl:NamedIndividual>
    


    <!-- http://purl.obolibrary.org/obo/GAZ_22223519 -->

    <owl:NamedIndividual rdf:about="http://purl.obolibrary.org/obo/GAZ_22223519">
        <obo:RO_0001025 rdf:resource="http://purl.obolibrary.org/obo/GAZ_00011612"/>
        <oboInOwl:hasOBONamespace>GAZ</oboInOwl:hasOBONamespace>
        <oboInOwl:id>GAZ:22223519</oboInOwl:id>
        <rdfs:label>Municipality of Jesus Maria Semprun</rdfs:label>
    </owl:NamedIndividual>
    


    <!-- http://purl.obolibrary.org/obo/GAZ_22223520 -->

    <owl:NamedIndividual rdf:about="http://purl.obolibrary.org/obo/GAZ_22223520">
        <obo:RO_0001025 rdf:resource="http://purl.obolibrary.org/obo/GAZ_00011612"/>
        <oboInOwl:hasOBONamespace>GAZ</oboInOwl:hasOBONamespace>
        <oboInOwl:id>GAZ:22223520</oboInOwl:id>
        <rdfs:label>Municipality of Paez</rdfs:label>
    </owl:NamedIndividual>
    


    <!-- http://purl.obolibrary.org/obo/GAZ_22223521 -->

    <owl:NamedIndividual rdf:about="http://purl.obolibrary.org/obo/GAZ_22223521">
        <obo:RO_0001025 rdf:resource="http://purl.obolibrary.org/obo/GAZ_00011612"/>
        <oboInOwl:hasOBONamespace>GAZ</oboInOwl:hasOBONamespace>
        <oboInOwl:id>GAZ:22223521</oboInOwl:id>
        <rdfs:label>Municipality of Sucre</rdfs:label>
    </owl:NamedIndividual>
    


    <!-- http://purl.obolibrary.org/obo/GAZ_22223522 -->

    <owl:NamedIndividual rdf:about="http://purl.obolibrary.org/obo/GAZ_22223522">
        <obo:RO_0001025 rdf:resource="http://purl.obolibrary.org/obo/GAZ_00011612"/>
        <oboInOwl:hasOBONamespace>GAZ</oboInOwl:hasOBONamespace>
        <oboInOwl:id>GAZ:22223522</oboInOwl:id>
        <rdfs:label>Municipality of La Canada de Urdaneta</rdfs:label>
    </owl:NamedIndividual>
    


    <!-- http://purl.obolibrary.org/obo/GAZ_22223523 -->

    <owl:NamedIndividual rdf:about="http://purl.obolibrary.org/obo/GAZ_22223523">
        <obo:RO_0001025 rdf:resource="http://purl.obolibrary.org/obo/GAZ_00011612"/>
        <oboInOwl:hasOBONamespace>GAZ</oboInOwl:hasOBONamespace>
        <oboInOwl:id>GAZ:22223523</oboInOwl:id>
        <rdfs:label>Municipality of Francisco Javier Pulgar</rdfs:label>
    </owl:NamedIndividual>
    


    <!-- http://purl.obolibrary.org/obo/GAZ_22223524 -->

    <owl:NamedIndividual rdf:about="http://purl.obolibrary.org/obo/GAZ_22223524">
        <obo:RO_0001025 rdf:resource="http://purl.obolibrary.org/obo/GAZ_00011612"/>
        <oboInOwl:hasOBONamespace>GAZ</oboInOwl:hasOBONamespace>
        <oboInOwl:id>GAZ:22223524</oboInOwl:id>
        <rdfs:label>Municipality of San Francisco</rdfs:label>
    </owl:NamedIndividual>
    


    <!-- http://purl.obolibrary.org/obo/GAZ_22223525 -->

    <owl:NamedIndividual rdf:about="http://purl.obolibrary.org/obo/GAZ_22223525">
        <obo:RO_0001025 rdf:resource="http://purl.obolibrary.org/obo/GAZ_00011612"/>
        <oboInOwl:hasOBONamespace>GAZ</oboInOwl:hasOBONamespace>
        <oboInOwl:id>GAZ:22223525</oboInOwl:id>
        <rdfs:label>Municipality of Santa Rita</rdfs:label>
    </owl:NamedIndividual>
    


    <!-- http://purl.obolibrary.org/obo/GAZ_22223526 -->

    <owl:NamedIndividual rdf:about="http://purl.obolibrary.org/obo/GAZ_22223526">
        <obo:RO_0001025 rdf:resource="http://purl.obolibrary.org/obo/GAZ_00011612"/>
        <oboInOwl:hasOBONamespace>GAZ</oboInOwl:hasOBONamespace>
        <oboInOwl:id>GAZ:22223526</oboInOwl:id>
        <rdfs:label>Municipality of Lagunillas</rdfs:label>
    </owl:NamedIndividual>
    


    <!-- http://purl.obolibrary.org/obo/GAZ_22223527 -->

    <owl:NamedIndividual rdf:about="http://purl.obolibrary.org/obo/GAZ_22223527">
        <obo:RO_0001025 rdf:resource="http://purl.obolibrary.org/obo/GAZ_00011612"/>
        <oboInOwl:hasOBONamespace>GAZ</oboInOwl:hasOBONamespace>
        <oboInOwl:id>GAZ:22223527</oboInOwl:id>
        <rdfs:label>Municipality of Machiques de Perija</rdfs:label>
    </owl:NamedIndividual>
    


    <!-- http://purl.obolibrary.org/obo/GAZ_22223528 -->

    <owl:NamedIndividual rdf:about="http://purl.obolibrary.org/obo/GAZ_22223528">
        <obo:RO_0001025 rdf:resource="http://purl.obolibrary.org/obo/GAZ_00011612"/>
        <oboInOwl:hasOBONamespace>GAZ</oboInOwl:hasOBONamespace>
        <oboInOwl:id>GAZ:22223528</oboInOwl:id>
        <rdfs:label>Municipality of Miranda</rdfs:label>
    </owl:NamedIndividual>
    


    <!-- http://purl.obolibrary.org/obo/GAZ_22223529 -->

    <owl:NamedIndividual rdf:about="http://purl.obolibrary.org/obo/GAZ_22223529">
        <obo:RO_0001025 rdf:resource="http://purl.obolibrary.org/obo/GAZ_00011612"/>
        <oboInOwl:hasOBONamespace>GAZ</oboInOwl:hasOBONamespace>
        <oboInOwl:id>GAZ:22223529</oboInOwl:id>
        <rdfs:label>Municipality of Maracaibo</rdfs:label>
    </owl:NamedIndividual>
    


    <!-- http://purl.obolibrary.org/obo/GAZ_22223530 -->

    <owl:NamedIndividual rdf:about="http://purl.obolibrary.org/obo/GAZ_22223530">
        <obo:RO_0001025 rdf:resource="http://purl.obolibrary.org/obo/GAZ_00011612"/>
        <oboInOwl:hasOBONamespace>GAZ</oboInOwl:hasOBONamespace>
        <oboInOwl:id>GAZ:22223530</oboInOwl:id>
        <rdfs:label>Municipality of Mara</rdfs:label>
    </owl:NamedIndividual>
    


    <!-- 
    ///////////////////////////////////////////////////////////////////////////////////////
    //
    // Annotations
    //
    ///////////////////////////////////////////////////////////////////////////////////////
     -->

    <rdf:Description rdf:about="http://purl.obolibrary.org/obo/GAZ_00009150">
        <rdfs:label>State (Venezuela)</rdfs:label>
        <oboInOwl:id>GAZ:00009150</oboInOwl:id>
        <oboInOwl:hasOBONamespace>GAZ</oboInOwl:hasOBONamespace>
    </rdf:Description>
    <rdf:Description rdf:about="http://purl.obolibrary.org/obo/GAZ_00009151">
        <obo:IAO_0000115>A State of Venezuela, located in the northeastern region of the country with a coast consisting of a single beach approximately 100 km long.</obo:IAO_0000115>
        <rdfs:label>Anzoategui State</rdfs:label>
        <oboInOwl:id>GAZ:00009151</oboInOwl:id>
        <oboInOwl:hasOBONamespace>GAZ</oboInOwl:hasOBONamespace>
    </rdf:Description>
    <rdf:Description rdf:about="http://purl.obolibrary.org/obo/GAZ_00009152">
        <oboInOwl:id>GAZ:00009152</oboInOwl:id>
        <rdfs:label>populated place, Venezuala</rdfs:label>
        <oboInOwl:hasOBONamespace>GAZ</oboInOwl:hasOBONamespace>
    </rdf:Description>
    <rdf:Description rdf:about="http://purl.obolibrary.org/obo/GAZ_00011584">
        <oboInOwl:id>GAZ:00011584</oboInOwl:id>
        <rdfs:label>Apure State</rdfs:label>
        <oboInOwl:hasOBONamespace>GAZ</oboInOwl:hasOBONamespace>
    </rdf:Description>
    <rdf:Description rdf:about="http://purl.obolibrary.org/obo/GAZ_00011585">
        <rdfs:label>Achaguas</rdfs:label>
        <oboInOwl:id>GAZ:00011585</oboInOwl:id>
        <oboInOwl:hasOBONamespace>GAZ</oboInOwl:hasOBONamespace>
    </rdf:Description>
    <rdf:Description rdf:about="http://purl.obolibrary.org/obo/GAZ_00011587">
        <oboInOwl:hasOBONamespace>GAZ</oboInOwl:hasOBONamespace>
        <oboInOwl:id>GAZ:00011587</oboInOwl:id>
        <rdfs:label>Aragua State</rdfs:label>
    </rdf:Description>
    <rdf:Description rdf:about="http://purl.obolibrary.org/obo/GAZ_00011588">
        <rdfs:label>Barinas State</rdfs:label>
        <oboInOwl:id>GAZ:00011588</oboInOwl:id>
        <oboInOwl:hasOBONamespace>GAZ</oboInOwl:hasOBONamespace>
    </rdf:Description>
    <rdf:Description rdf:about="http://purl.obolibrary.org/obo/GAZ_00011591">
        <oboInOwl:hasOBONamespace>GAZ</oboInOwl:hasOBONamespace>
        <rdfs:label>Caracas</rdfs:label>
        <oboInOwl:id>GAZ:00011591</oboInOwl:id>
    </rdf:Description>
    <rdf:Description rdf:about="http://purl.obolibrary.org/obo/GAZ_00011592">
        <rdfs:label>Cojedes State</rdfs:label>
        <oboInOwl:hasOBONamespace>GAZ</oboInOwl:hasOBONamespace>
        <oboInOwl:id>GAZ:00011592</oboInOwl:id>
    </rdf:Description>
    <rdf:Description rdf:about="http://purl.obolibrary.org/obo/GAZ_00011593">
        <oboInOwl:hasOBONamespace>GAZ</oboInOwl:hasOBONamespace>
        <rdfs:label>Cojedes</rdfs:label>
        <oboInOwl:id>GAZ:00011593</oboInOwl:id>
    </rdf:Description>
    <rdf:Description rdf:about="http://purl.obolibrary.org/obo/GAZ_00011595">
        <oboInOwl:id>GAZ:00011595</oboInOwl:id>
        <rdfs:label>Guarico State</rdfs:label>
        <oboInOwl:hasOBONamespace>GAZ</oboInOwl:hasOBONamespace>
    </rdf:Description>
    <rdf:Description rdf:about="http://purl.obolibrary.org/obo/GAZ_00011598">
        <oboInOwl:id>GAZ:00011598</oboInOwl:id>
        <rdfs:label>Portuguesa State</rdfs:label>
        <oboInOwl:hasOBONamespace>GAZ</oboInOwl:hasOBONamespace>
    </rdf:Description>
    <rdf:Description rdf:about="http://purl.obolibrary.org/obo/GAZ_00011603">
        <oboInOwl:hasOBONamespace>GAZ</oboInOwl:hasOBONamespace>
        <rdfs:label>Guanare</rdfs:label>
        <oboInOwl:id>GAZ:00011603</oboInOwl:id>
    </rdf:Description>
    <rdf:Description rdf:about="http://purl.obolibrary.org/obo/GAZ_00011608">
        <rdfs:label>La Rompia</rdfs:label>
        <oboInOwl:id>GAZ:00011608</oboInOwl:id>
        <oboInOwl:hasOBONamespace>GAZ</oboInOwl:hasOBONamespace>
    </rdf:Description>
    <rdf:Description rdf:about="http://purl.obolibrary.org/obo/GAZ_00011612">
        <rdfs:label>Zulia State</rdfs:label>
        <obo:IAO_0000115>A state in Venezuela located in the northwestern part of the country with the largest population among Venzuela&apos;s states, covers a total surface area of 63,100 km2.</obo:IAO_0000115>
        <oboInOwl:hasOBONamespace>GAZ</oboInOwl:hasOBONamespace>
        <oboInOwl:id>GAZ:00011612</oboInOwl:id>
    </rdf:Description>
    <rdf:Description rdf:about="http://purl.obolibrary.org/obo/GAZ_00011614">
        <oboInOwl:hasOBONamespace>GAZ</oboInOwl:hasOBONamespace>
        <oboInOwl:id>GAZ:00011614</oboInOwl:id>
        <rdfs:label>Falcon State</rdfs:label>
    </rdf:Description>
    <rdf:Description rdf:about="http://purl.obolibrary.org/obo/GAZ_00011615">
        <oboInOwl:hasOBONamespace>GAZ</oboInOwl:hasOBONamespace>
        <rdfs:label>Bolivar State</rdfs:label>
        <oboInOwl:id>GAZ:00011615</oboInOwl:id>
    </rdf:Description>
    <rdf:Description rdf:about="http://purl.obolibrary.org/obo/GAZ_00011616">
        <oboInOwl:hasOBONamespace>GAZ</oboInOwl:hasOBONamespace>
        <oboInOwl:id>GAZ:00011616</oboInOwl:id>
        <rdfs:label>Carabobo State</rdfs:label>
    </rdf:Description>
    <rdf:Description rdf:about="http://purl.obolibrary.org/obo/GAZ_00011617">
        <oboInOwl:hasOBONamespace>GAZ</oboInOwl:hasOBONamespace>
        <oboInOwl:id>GAZ:00011617</oboInOwl:id>
        <rdfs:label>Delta Amacuro State</rdfs:label>
    </rdf:Description>
    <rdf:Description rdf:about="http://purl.obolibrary.org/obo/GAZ_00011618">
        <rdfs:label>Amazonas State</rdfs:label>
        <oboInOwl:id>GAZ:00011618</oboInOwl:id>
        <oboInOwl:hasOBONamespace>GAZ</oboInOwl:hasOBONamespace>
    </rdf:Description>
    <rdf:Description rdf:about="http://purl.obolibrary.org/obo/GAZ_00011620">
        <rdfs:label>Monagas State</rdfs:label>
        <oboInOwl:id>GAZ:00011620</oboInOwl:id>
        <oboInOwl:hasOBONamespace>GAZ</oboInOwl:hasOBONamespace>
    </rdf:Description>
    <rdf:Description rdf:about="http://purl.obolibrary.org/obo/GAZ_00011621">
        <oboInOwl:id>GAZ:00011621</oboInOwl:id>
        <oboInOwl:hasOBONamespace>GAZ</oboInOwl:hasOBONamespace>
        <rdfs:label>Merida State</rdfs:label>
    </rdf:Description>
    <rdf:Description rdf:about="http://purl.obolibrary.org/obo/GAZ_00011622">
        <oboInOwl:hasOBONamespace>GAZ</oboInOwl:hasOBONamespace>
        <rdfs:label>Miranda State</rdfs:label>
        <oboInOwl:id>GAZ:00011622</oboInOwl:id>
    </rdf:Description>
    <rdf:Description rdf:about="http://purl.obolibrary.org/obo/GAZ_00011623">
        <rdfs:label>Lara State</rdfs:label>
        <oboInOwl:id>GAZ:00011623</oboInOwl:id>
        <oboInOwl:hasOBONamespace>GAZ</oboInOwl:hasOBONamespace>
    </rdf:Description>
    <rdf:Description rdf:about="http://purl.obolibrary.org/obo/GAZ_00011624">
        <rdfs:label>Trujillo State</rdfs:label>
        <oboInOwl:id>GAZ:00011624</oboInOwl:id>
        <oboInOwl:hasOBONamespace>GAZ</oboInOwl:hasOBONamespace>
    </rdf:Description>
    <rdf:Description rdf:about="http://purl.obolibrary.org/obo/GAZ_00011625">
        <oboInOwl:hasOBONamespace>GAZ</oboInOwl:hasOBONamespace>
        <rdfs:label>Tachira State</rdfs:label>
        <oboInOwl:id>GAZ:00011625</oboInOwl:id>
    </rdf:Description>
    <rdf:Description rdf:about="http://purl.obolibrary.org/obo/GAZ_00011626">
        <oboInOwl:hasOBONamespace>GAZ</oboInOwl:hasOBONamespace>
        <rdfs:label>Sucre State</rdfs:label>
        <oboInOwl:id>GAZ:00011626</oboInOwl:id>
    </rdf:Description>
    <rdf:Description rdf:about="http://purl.obolibrary.org/obo/GAZ_00011627">
        <oboInOwl:hasOBONamespace>GAZ</oboInOwl:hasOBONamespace>
        <oboInOwl:id>GAZ:00011627</oboInOwl:id>
        <rdfs:label>Nueva Esparta State</rdfs:label>
    </rdf:Description>
    <rdf:Description rdf:about="http://purl.obolibrary.org/obo/GAZ_00011628">
        <oboInOwl:hasOBONamespace>GAZ</oboInOwl:hasOBONamespace>
        <rdfs:label>Yaracuy State</rdfs:label>
        <oboInOwl:id>GAZ:00011628</oboInOwl:id>
    </rdf:Description>
    <rdf:Description rdf:about="http://purl.obolibrary.org/obo/GAZ_00011629">
        <rdfs:label>Vargas State</rdfs:label>
        <oboInOwl:id>GAZ:00011629</oboInOwl:id>
        <oboInOwl:hasOBONamespace>GAZ</oboInOwl:hasOBONamespace>
    </rdf:Description>
    <rdf:Description rdf:about="http://purl.obolibrary.org/obo/GAZ_02000849">
        <rdfs:label>Guanta</rdfs:label>
        <oboInOwl:hasOBONamespace>GAZ</oboInOwl:hasOBONamespace>
        <oboInOwl:id>GAZ:02000849</oboInOwl:id>
    </rdf:Description>
</rdf:RDF>



<!-- Generated by the OWL API (version 4.5.6) https://github.com/owlcs/owlapi -->

