<?xml version="1.0"?>
<rdf:RDF xmlns="http://purl.obolibrary.org/obo/gaz/subsets/countries/Zambia.owl#"
     xml:base="http://purl.obolibrary.org/obo/gaz/subsets/countries/Zambia.owl"
     xmlns:obo="http://purl.obolibrary.org/obo/"
     xmlns:owl="http://www.w3.org/2002/07/owl#"
     xmlns:rdf="http://www.w3.org/1999/02/22-rdf-syntax-ns#"
     xmlns:xml="http://www.w3.org/XML/1998/namespace"
     xmlns:xsd="http://www.w3.org/2001/XMLSchema#"
     xmlns:rdfs="http://www.w3.org/2000/01/rdf-schema#"
     xmlns:oboInOwl="http://www.geneontology.org/formats/oboInOwl#">
    <owl:Ontology rdf:about="http://purl.obolibrary.org/obo/gaz/subsets/countries/Zambia.owl">
        <owl:imports rdf:resource="http://purl.obolibrary.org/obo/gaz/imports/envo_import.owl"/>
        <owl:imports rdf:resource="http://purl.obolibrary.org/obo/gaz/imports/ro_import.owl"/>
    </owl:Ontology>
    


    <!-- 
    ///////////////////////////////////////////////////////////////////////////////////////
    //
    // Annotation properties
    //
    ///////////////////////////////////////////////////////////////////////////////////////
     -->

    


    <!-- http://purl.obolibrary.org/obo/IAO_0000115 -->

    <owl:AnnotationProperty rdf:about="http://purl.obolibrary.org/obo/IAO_0000115"/>
    


    <!-- http://www.geneontology.org/formats/oboInOwl#hasOBONamespace -->

    <owl:AnnotationProperty rdf:about="http://www.geneontology.org/formats/oboInOwl#hasOBONamespace"/>
    


    <!-- http://www.geneontology.org/formats/oboInOwl#id -->

    <owl:AnnotationProperty rdf:about="http://www.geneontology.org/formats/oboInOwl#id"/>
    


    <!-- 
    ///////////////////////////////////////////////////////////////////////////////////////
    //
    // Object Properties
    //
    ///////////////////////////////////////////////////////////////////////////////////////
     -->

    


    <!-- http://purl.obolibrary.org/obo/RO_0001025 -->

    <owl:ObjectProperty rdf:about="http://purl.obolibrary.org/obo/RO_0001025"/>
    


    <!-- 
    ///////////////////////////////////////////////////////////////////////////////////////
    //
    // Classes
    //
    ///////////////////////////////////////////////////////////////////////////////////////
     -->

    


    <!-- http://purl.obolibrary.org/obo/ENVO_00000004 -->

    <owl:Class rdf:about="http://purl.obolibrary.org/obo/ENVO_00000004"/>
    


    <!-- http://purl.obolibrary.org/obo/ENVO_00000062 -->

    <owl:Class rdf:about="http://purl.obolibrary.org/obo/ENVO_00000062"/>
    


    <!-- http://purl.obolibrary.org/obo/ENVO_00000856 -->

    <owl:Class rdf:about="http://purl.obolibrary.org/obo/ENVO_00000856"/>
    


    <!-- http://purl.obolibrary.org/obo/GAZ_00009419 -->

    <owl:Class rdf:about="http://purl.obolibrary.org/obo/GAZ_00009419"/>
    


    <!-- http://purl.obolibrary.org/obo/GAZ_00009420 -->

    <owl:Class rdf:about="http://purl.obolibrary.org/obo/GAZ_00009420">
        <rdfs:subClassOf rdf:resource="http://purl.obolibrary.org/obo/GAZ_00009419"/>
    </owl:Class>
    


    <!-- http://purl.obolibrary.org/obo/GAZ_00009421 -->

    <owl:Class rdf:about="http://purl.obolibrary.org/obo/GAZ_00009421">
        <rdfs:subClassOf rdf:resource="http://purl.obolibrary.org/obo/GAZ_00009419"/>
    </owl:Class>
    


    <!-- http://purl.obolibrary.org/obo/GAZ_00009422 -->

    <owl:Class rdf:about="http://purl.obolibrary.org/obo/GAZ_00009422">
        <rdfs:subClassOf rdf:resource="http://purl.obolibrary.org/obo/GAZ_00009419"/>
    </owl:Class>
    


    <!-- http://purl.obolibrary.org/obo/GAZ_00009423 -->

    <owl:Class rdf:about="http://purl.obolibrary.org/obo/GAZ_00009423">
        <rdfs:subClassOf rdf:resource="http://purl.obolibrary.org/obo/GAZ_00009419"/>
    </owl:Class>
    


    <!-- http://purl.obolibrary.org/obo/GAZ_00009425 -->

    <owl:Class rdf:about="http://purl.obolibrary.org/obo/GAZ_00009425">
        <rdfs:subClassOf rdf:resource="http://purl.obolibrary.org/obo/GAZ_00009419"/>
    </owl:Class>
    


    <!-- http://purl.obolibrary.org/obo/GAZ_00009427 -->

    <owl:Class rdf:about="http://purl.obolibrary.org/obo/GAZ_00009427">
        <rdfs:subClassOf rdf:resource="http://purl.obolibrary.org/obo/GAZ_00009419"/>
    </owl:Class>
    


    <!-- http://purl.obolibrary.org/obo/GAZ_00009428 -->

    <owl:Class rdf:about="http://purl.obolibrary.org/obo/GAZ_00009428">
        <rdfs:subClassOf rdf:resource="http://purl.obolibrary.org/obo/GAZ_00009419"/>
    </owl:Class>
    


    <!-- http://purl.obolibrary.org/obo/GAZ_00009429 -->

    <owl:Class rdf:about="http://purl.obolibrary.org/obo/GAZ_00009429">
        <rdfs:subClassOf rdf:resource="http://purl.obolibrary.org/obo/GAZ_00009419"/>
    </owl:Class>
    


    <!-- http://purl.obolibrary.org/obo/GAZ_00009430 -->

    <owl:Class rdf:about="http://purl.obolibrary.org/obo/GAZ_00009430">
        <rdfs:subClassOf rdf:resource="http://purl.obolibrary.org/obo/GAZ_00009419"/>
    </owl:Class>
    


    <!-- http://purl.obolibrary.org/obo/GAZ_00010009 -->

    <owl:Class rdf:about="http://purl.obolibrary.org/obo/GAZ_00010009">
        <rdfs:subClassOf rdf:resource="http://purl.obolibrary.org/obo/GAZ_00010010"/>
    </owl:Class>
    


    <!-- http://purl.obolibrary.org/obo/GAZ_00010010 -->

    <owl:Class rdf:about="http://purl.obolibrary.org/obo/GAZ_00010010"/>
    


    <!-- http://purl.obolibrary.org/obo/GAZ_00010011 -->

    <owl:Class rdf:about="http://purl.obolibrary.org/obo/GAZ_00010011">
        <rdfs:subClassOf rdf:resource="http://purl.obolibrary.org/obo/GAZ_00010010"/>
    </owl:Class>
    


    <!-- http://purl.obolibrary.org/obo/GAZ_00052622 -->

    <owl:Class rdf:about="http://purl.obolibrary.org/obo/GAZ_00052622">
        <rdfs:subClassOf rdf:resource="http://purl.obolibrary.org/obo/GAZ_00010010"/>
    </owl:Class>
    


    <!-- http://purl.obolibrary.org/obo/GAZ_00052623 -->

    <owl:Class rdf:about="http://purl.obolibrary.org/obo/GAZ_00052623">
        <rdfs:subClassOf rdf:resource="http://purl.obolibrary.org/obo/GAZ_00010010"/>
    </owl:Class>
    


    <!-- http://purl.obolibrary.org/obo/GAZ_00052624 -->

    <owl:Class rdf:about="http://purl.obolibrary.org/obo/GAZ_00052624">
        <rdfs:subClassOf rdf:resource="http://purl.obolibrary.org/obo/GAZ_00010010"/>
    </owl:Class>
    


    <!-- http://purl.obolibrary.org/obo/GAZ_00052625 -->

    <owl:Class rdf:about="http://purl.obolibrary.org/obo/GAZ_00052625">
        <rdfs:subClassOf rdf:resource="http://purl.obolibrary.org/obo/GAZ_00010010"/>
    </owl:Class>
    


    <!-- http://purl.obolibrary.org/obo/GAZ_00052628 -->

    <owl:Class rdf:about="http://purl.obolibrary.org/obo/GAZ_00052628">
        <rdfs:subClassOf rdf:resource="http://purl.obolibrary.org/obo/GAZ_00010010"/>
    </owl:Class>
    


    <!-- http://purl.obolibrary.org/obo/GAZ_00052631 -->

    <owl:Class rdf:about="http://purl.obolibrary.org/obo/GAZ_00052631">
        <rdfs:subClassOf rdf:resource="http://purl.obolibrary.org/obo/GAZ_00010010"/>
    </owl:Class>
    


    <!-- http://purl.obolibrary.org/obo/GAZ_00052641 -->

    <owl:Class rdf:about="http://purl.obolibrary.org/obo/GAZ_00052641">
        <rdfs:subClassOf rdf:resource="http://purl.obolibrary.org/obo/GAZ_00010010"/>
    </owl:Class>
    


    <!-- http://purl.obolibrary.org/obo/GAZ_00052643 -->

    <owl:Class rdf:about="http://purl.obolibrary.org/obo/GAZ_00052643">
        <rdfs:subClassOf rdf:resource="http://purl.obolibrary.org/obo/GAZ_00010010"/>
    </owl:Class>
    


    <!-- http://purl.obolibrary.org/obo/GAZ_00052644 -->

    <owl:Class rdf:about="http://purl.obolibrary.org/obo/GAZ_00052644">
        <rdfs:subClassOf rdf:resource="http://purl.obolibrary.org/obo/GAZ_00010010"/>
    </owl:Class>
    


    <!-- http://purl.obolibrary.org/obo/GAZ_00052645 -->

    <owl:Class rdf:about="http://purl.obolibrary.org/obo/GAZ_00052645">
        <rdfs:subClassOf rdf:resource="http://purl.obolibrary.org/obo/GAZ_00010010"/>
    </owl:Class>
    


    <!-- http://purl.obolibrary.org/obo/GAZ_00052647 -->

    <owl:Class rdf:about="http://purl.obolibrary.org/obo/GAZ_00052647">
        <rdfs:subClassOf rdf:resource="http://purl.obolibrary.org/obo/GAZ_00010010"/>
    </owl:Class>
    


    <!-- http://purl.obolibrary.org/obo/GAZ_00052651 -->

    <owl:Class rdf:about="http://purl.obolibrary.org/obo/GAZ_00052651">
        <rdfs:subClassOf rdf:resource="http://purl.obolibrary.org/obo/GAZ_00010010"/>
    </owl:Class>
    


    <!-- http://purl.obolibrary.org/obo/GAZ_00052654 -->

    <owl:Class rdf:about="http://purl.obolibrary.org/obo/GAZ_00052654">
        <rdfs:subClassOf rdf:resource="http://purl.obolibrary.org/obo/GAZ_00010010"/>
    </owl:Class>
    


    <!-- http://purl.obolibrary.org/obo/GAZ_00052655 -->

    <owl:Class rdf:about="http://purl.obolibrary.org/obo/GAZ_00052655">
        <rdfs:subClassOf rdf:resource="http://purl.obolibrary.org/obo/GAZ_00010010"/>
    </owl:Class>
    


    <!-- http://purl.obolibrary.org/obo/GAZ_00052656 -->

    <owl:Class rdf:about="http://purl.obolibrary.org/obo/GAZ_00052656">
        <rdfs:subClassOf rdf:resource="http://purl.obolibrary.org/obo/GAZ_00010010"/>
    </owl:Class>
    


    <!-- http://purl.obolibrary.org/obo/GAZ_00052661 -->

    <owl:Class rdf:about="http://purl.obolibrary.org/obo/GAZ_00052661">
        <rdfs:subClassOf rdf:resource="http://purl.obolibrary.org/obo/GAZ_00010010"/>
    </owl:Class>
    


    <!-- 
    ///////////////////////////////////////////////////////////////////////////////////////
    //
    // Individuals
    //
    ///////////////////////////////////////////////////////////////////////////////////////
     -->

    


    <!-- http://purl.obolibrary.org/obo/GAZ_00001107 -->

    <owl:NamedIndividual rdf:about="http://purl.obolibrary.org/obo/GAZ_00001107">
        <obo:IAO_0000115>A landlocked country in Southern Africa. The neighbouring countries are the Democratic Republic of the Congo to the north, Tanzania to the north-east, Malawi to the east, Mozambique, Zimbabwe, Botswana, and Namibia to the south, and Angola to the west. The capital city is Lusaka. Zambia is divided into nine provinces. Each province is subdivided into several districts with a total of 73 districts.</obo:IAO_0000115>
        <oboInOwl:hasOBONamespace>GAZ</oboInOwl:hasOBONamespace>
        <oboInOwl:id>GAZ:00001107</oboInOwl:id>
        <rdfs:label>Zambia</rdfs:label>
    </owl:NamedIndividual>
    


    <!-- http://purl.obolibrary.org/obo/GAZ_00005134 -->

    <owl:NamedIndividual rdf:about="http://purl.obolibrary.org/obo/GAZ_00005134">
        <obo:RO_0001025 rdf:resource="http://purl.obolibrary.org/obo/GAZ_00044898"/>
        <obo:IAO_0000115>A waterfall on the Zambezi River.</obo:IAO_0000115>
        <oboInOwl:hasOBONamespace>GAZ</oboInOwl:hasOBONamespace>
        <oboInOwl:id>GAZ:00005134</oboInOwl:id>
        <rdfs:label>Victoria Falls</rdfs:label>
    </owl:NamedIndividual>
    


    <!-- http://purl.obolibrary.org/obo/GAZ_00009419 -->

    <owl:NamedIndividual rdf:about="http://purl.obolibrary.org/obo/GAZ_00009419">
        <obo:RO_0001025 rdf:resource="http://purl.obolibrary.org/obo/GAZ_00001107"/>
    </owl:NamedIndividual>
    


    <!-- http://purl.obolibrary.org/obo/GAZ_00009420 -->

    <owl:NamedIndividual rdf:about="http://purl.obolibrary.org/obo/GAZ_00009420"/>
    


    <!-- http://purl.obolibrary.org/obo/GAZ_00009421 -->

    <owl:NamedIndividual rdf:about="http://purl.obolibrary.org/obo/GAZ_00009421"/>
    


    <!-- http://purl.obolibrary.org/obo/GAZ_00009422 -->

    <owl:NamedIndividual rdf:about="http://purl.obolibrary.org/obo/GAZ_00009422"/>
    


    <!-- http://purl.obolibrary.org/obo/GAZ_00009423 -->

    <owl:NamedIndividual rdf:about="http://purl.obolibrary.org/obo/GAZ_00009423"/>
    


    <!-- http://purl.obolibrary.org/obo/GAZ_00009425 -->

    <owl:NamedIndividual rdf:about="http://purl.obolibrary.org/obo/GAZ_00009425"/>
    


    <!-- http://purl.obolibrary.org/obo/GAZ_00009427 -->

    <owl:NamedIndividual rdf:about="http://purl.obolibrary.org/obo/GAZ_00009427"/>
    


    <!-- http://purl.obolibrary.org/obo/GAZ_00009428 -->

    <owl:NamedIndividual rdf:about="http://purl.obolibrary.org/obo/GAZ_00009428"/>
    


    <!-- http://purl.obolibrary.org/obo/GAZ_00009429 -->

    <owl:NamedIndividual rdf:about="http://purl.obolibrary.org/obo/GAZ_00009429"/>
    


    <!-- http://purl.obolibrary.org/obo/GAZ_00009430 -->

    <owl:NamedIndividual rdf:about="http://purl.obolibrary.org/obo/GAZ_00009430"/>
    


    <!-- http://purl.obolibrary.org/obo/GAZ_00010009 -->

    <owl:NamedIndividual rdf:about="http://purl.obolibrary.org/obo/GAZ_00010009">
        <obo:RO_0001025 rdf:resource="http://purl.obolibrary.org/obo/GAZ_04000027"/>
    </owl:NamedIndividual>
    


    <!-- http://purl.obolibrary.org/obo/GAZ_00010010 -->

    <owl:NamedIndividual rdf:about="http://purl.obolibrary.org/obo/GAZ_00010010">
        <rdf:type rdf:resource="http://purl.obolibrary.org/obo/ENVO_00000856"/>
        <obo:RO_0001025 rdf:resource="http://purl.obolibrary.org/obo/GAZ_00001107"/>
    </owl:NamedIndividual>
    


    <!-- http://purl.obolibrary.org/obo/GAZ_00010011 -->

    <owl:NamedIndividual rdf:about="http://purl.obolibrary.org/obo/GAZ_00010011">
        <obo:RO_0001025 rdf:resource="http://purl.obolibrary.org/obo/GAZ_04000028"/>
    </owl:NamedIndividual>
    


    <!-- http://purl.obolibrary.org/obo/GAZ_00011722 -->

    <owl:NamedIndividual rdf:about="http://purl.obolibrary.org/obo/GAZ_00011722">
        <obo:IAO_0000115>A freshwater lake is situated within the Western Rift of the Great Rift Valley. The major inflows are the Ruzizi River, entering the north of the lake from Lake Kivu, and the Malagarasi River, which is Tanzania&apos;s second largest river, entering in the east side of Lake Tanganyika. The Malagarasi pre-dates Lake Tanganyika and was formerly continuous with the Congo river.</obo:IAO_0000115>
        <oboInOwl:hasOBONamespace>GAZ</oboInOwl:hasOBONamespace>
        <oboInOwl:id>GAZ:00011722</oboInOwl:id>
        <rdfs:label>Lake Tanganyika</rdfs:label>
    </owl:NamedIndividual>
    


    <!-- http://purl.obolibrary.org/obo/GAZ_00015133 -->

    <owl:NamedIndividual rdf:about="http://purl.obolibrary.org/obo/GAZ_00015133">
        <obo:RO_0001025 rdf:resource="http://purl.obolibrary.org/obo/GAZ_00009429"/>
        <obo:IAO_0000115>An administrative district of Central Province.</obo:IAO_0000115>
        <oboInOwl:hasOBONamespace>GAZ</oboInOwl:hasOBONamespace>
        <oboInOwl:id>GAZ:00015133</oboInOwl:id>
        <rdfs:label>Mumbwa District</rdfs:label>
    </owl:NamedIndividual>
    


    <!-- http://purl.obolibrary.org/obo/GAZ_00015134 -->

    <owl:NamedIndividual rdf:about="http://purl.obolibrary.org/obo/GAZ_00015134">
        <obo:RO_0001025 rdf:resource="http://purl.obolibrary.org/obo/GAZ_00009429"/>
        <obo:IAO_0000115>An administrative district of Central Province.</obo:IAO_0000115>
        <oboInOwl:hasOBONamespace>GAZ</oboInOwl:hasOBONamespace>
        <oboInOwl:id>GAZ:00015134</oboInOwl:id>
        <rdfs:label>Kapiri Mposhi District</rdfs:label>
    </owl:NamedIndividual>
    


    <!-- http://purl.obolibrary.org/obo/GAZ_00015135 -->

    <owl:NamedIndividual rdf:about="http://purl.obolibrary.org/obo/GAZ_00015135">
        <obo:RO_0001025 rdf:resource="http://purl.obolibrary.org/obo/GAZ_00009429"/>
        <obo:IAO_0000115>An administrative district of Central Province. It lies between the Lukanga Swamp in the west and the end of the Luangwa Valley in the east.</obo:IAO_0000115>
        <oboInOwl:hasOBONamespace>GAZ</oboInOwl:hasOBONamespace>
        <oboInOwl:id>GAZ:00015135</oboInOwl:id>
        <rdfs:label>Serenje District</rdfs:label>
    </owl:NamedIndividual>
    


    <!-- http://purl.obolibrary.org/obo/GAZ_00015136 -->

    <owl:NamedIndividual rdf:about="http://purl.obolibrary.org/obo/GAZ_00015136">
        <obo:RO_0001025 rdf:resource="http://purl.obolibrary.org/obo/GAZ_00009429"/>
        <obo:IAO_0000115>An administrative district of Central Province.</obo:IAO_0000115>
        <oboInOwl:hasOBONamespace>GAZ</oboInOwl:hasOBONamespace>
        <oboInOwl:id>GAZ:00015136</oboInOwl:id>
        <rdfs:label>Mkushi District</rdfs:label>
    </owl:NamedIndividual>
    


    <!-- http://purl.obolibrary.org/obo/GAZ_00015137 -->

    <owl:NamedIndividual rdf:about="http://purl.obolibrary.org/obo/GAZ_00015137">
        <obo:RO_0001025 rdf:resource="http://purl.obolibrary.org/obo/GAZ_00009429"/>
        <obo:IAO_0000115>An administrative district of Central Province.</obo:IAO_0000115>
        <oboInOwl:hasOBONamespace>GAZ</oboInOwl:hasOBONamespace>
        <oboInOwl:id>GAZ:00015137</oboInOwl:id>
        <rdfs:label>Kabwe District</rdfs:label>
    </owl:NamedIndividual>
    


    <!-- http://purl.obolibrary.org/obo/GAZ_00015138 -->

    <owl:NamedIndividual rdf:about="http://purl.obolibrary.org/obo/GAZ_00015138">
        <obo:RO_0001025 rdf:resource="http://purl.obolibrary.org/obo/GAZ_00009429"/>
        <obo:IAO_0000115>An administrative district of Central Province.</obo:IAO_0000115>
        <oboInOwl:hasOBONamespace>GAZ</oboInOwl:hasOBONamespace>
        <oboInOwl:id>GAZ:00015138</oboInOwl:id>
        <rdfs:label>Chibombo District</rdfs:label>
    </owl:NamedIndividual>
    


    <!-- http://purl.obolibrary.org/obo/GAZ_00015139 -->

    <owl:NamedIndividual rdf:about="http://purl.obolibrary.org/obo/GAZ_00015139">
        <rdf:type rdf:resource="http://purl.obolibrary.org/obo/ENVO_00000004"/>
        <obo:RO_0001025 rdf:resource="http://purl.obolibrary.org/obo/GAZ_00009425"/>
        <obo:IAO_0000115>A district of Copperbelt Province.</obo:IAO_0000115>
        <oboInOwl:hasOBONamespace>GAZ</oboInOwl:hasOBONamespace>
        <oboInOwl:id>GAZ:00015139</oboInOwl:id>
        <rdfs:label>Chililabombwe District</rdfs:label>
    </owl:NamedIndividual>
    


    <!-- http://purl.obolibrary.org/obo/GAZ_00015140 -->

    <owl:NamedIndividual rdf:about="http://purl.obolibrary.org/obo/GAZ_00015140">
        <obo:RO_0001025 rdf:resource="http://purl.obolibrary.org/obo/GAZ_00009421"/>
        <obo:IAO_0000115>A District located in the Eastern Province of Zambia.</obo:IAO_0000115>
        <oboInOwl:hasOBONamespace>GAZ</oboInOwl:hasOBONamespace>
        <oboInOwl:id>GAZ:00015140</oboInOwl:id>
        <rdfs:label>Chipata District</rdfs:label>
    </owl:NamedIndividual>
    


    <!-- http://purl.obolibrary.org/obo/GAZ_00015141 -->

    <owl:NamedIndividual rdf:about="http://purl.obolibrary.org/obo/GAZ_00015141">
        <rdf:type rdf:resource="http://purl.obolibrary.org/obo/ENVO_00000004"/>
        <obo:RO_0001025 rdf:resource="http://purl.obolibrary.org/obo/GAZ_00009425"/>
        <obo:IAO_0000115>A district of Copperbelt Province.</obo:IAO_0000115>
        <oboInOwl:hasOBONamespace>GAZ</oboInOwl:hasOBONamespace>
        <oboInOwl:id>GAZ:00015141</oboInOwl:id>
        <rdfs:label>Ndola District</rdfs:label>
    </owl:NamedIndividual>
    


    <!-- http://purl.obolibrary.org/obo/GAZ_00015142 -->

    <owl:NamedIndividual rdf:about="http://purl.obolibrary.org/obo/GAZ_00015142">
        <rdf:type rdf:resource="http://purl.obolibrary.org/obo/ENVO_00000004"/>
        <obo:RO_0001025 rdf:resource="http://purl.obolibrary.org/obo/GAZ_00009425"/>
        <obo:IAO_0000115>A district of Copperbelt Province.</obo:IAO_0000115>
        <oboInOwl:hasOBONamespace>GAZ</oboInOwl:hasOBONamespace>
        <oboInOwl:id>GAZ:00015142</oboInOwl:id>
        <rdfs:label>Kalulushi District</rdfs:label>
    </owl:NamedIndividual>
    


    <!-- http://purl.obolibrary.org/obo/GAZ_00015143 -->

    <owl:NamedIndividual rdf:about="http://purl.obolibrary.org/obo/GAZ_00015143">
        <rdf:type rdf:resource="http://purl.obolibrary.org/obo/ENVO_00000004"/>
        <obo:RO_0001025 rdf:resource="http://purl.obolibrary.org/obo/GAZ_00009425"/>
        <obo:IAO_0000115>A district of Copperbelt Province.</obo:IAO_0000115>
        <oboInOwl:hasOBONamespace>GAZ</oboInOwl:hasOBONamespace>
        <oboInOwl:id>GAZ:00015143</oboInOwl:id>
        <rdfs:label>Mufulira District</rdfs:label>
    </owl:NamedIndividual>
    


    <!-- http://purl.obolibrary.org/obo/GAZ_00015144 -->

    <owl:NamedIndividual rdf:about="http://purl.obolibrary.org/obo/GAZ_00015144">
        <rdf:type rdf:resource="http://purl.obolibrary.org/obo/ENVO_00000004"/>
        <obo:RO_0001025 rdf:resource="http://purl.obolibrary.org/obo/GAZ_00009425"/>
        <obo:IAO_0000115>A district of Copperbelt Province.</obo:IAO_0000115>
        <oboInOwl:hasOBONamespace>GAZ</oboInOwl:hasOBONamespace>
        <oboInOwl:id>GAZ:00015144</oboInOwl:id>
        <rdfs:label>Kitwe District</rdfs:label>
    </owl:NamedIndividual>
    


    <!-- http://purl.obolibrary.org/obo/GAZ_00015145 -->

    <owl:NamedIndividual rdf:about="http://purl.obolibrary.org/obo/GAZ_00015145">
        <rdf:type rdf:resource="http://purl.obolibrary.org/obo/ENVO_00000004"/>
        <obo:RO_0001025 rdf:resource="http://purl.obolibrary.org/obo/GAZ_00009425"/>
        <obo:IAO_0000115>A district of Copperbelt Province.</obo:IAO_0000115>
        <oboInOwl:hasOBONamespace>GAZ</oboInOwl:hasOBONamespace>
        <oboInOwl:id>GAZ:00015145</oboInOwl:id>
        <rdfs:label>Lufwanyama District</rdfs:label>
    </owl:NamedIndividual>
    


    <!-- http://purl.obolibrary.org/obo/GAZ_00015146 -->

    <owl:NamedIndividual rdf:about="http://purl.obolibrary.org/obo/GAZ_00015146">
        <rdf:type rdf:resource="http://purl.obolibrary.org/obo/ENVO_00000004"/>
        <obo:RO_0001025 rdf:resource="http://purl.obolibrary.org/obo/GAZ_00009425"/>
        <obo:IAO_0000115>A district of Copperbelt Province.</obo:IAO_0000115>
        <oboInOwl:hasOBONamespace>GAZ</oboInOwl:hasOBONamespace>
        <oboInOwl:id>GAZ:00015146</oboInOwl:id>
        <rdfs:label>Luanshya District</rdfs:label>
    </owl:NamedIndividual>
    


    <!-- http://purl.obolibrary.org/obo/GAZ_00015147 -->

    <owl:NamedIndividual rdf:about="http://purl.obolibrary.org/obo/GAZ_00015147">
        <rdf:type rdf:resource="http://purl.obolibrary.org/obo/ENVO_00000004"/>
        <obo:RO_0001025 rdf:resource="http://purl.obolibrary.org/obo/GAZ_00009425"/>
        <obo:IAO_0000115>A district of Copperbelt Province.</obo:IAO_0000115>
        <oboInOwl:hasOBONamespace>GAZ</oboInOwl:hasOBONamespace>
        <oboInOwl:id>GAZ:00015147</oboInOwl:id>
        <rdfs:label>Mpongwe District</rdfs:label>
    </owl:NamedIndividual>
    


    <!-- http://purl.obolibrary.org/obo/GAZ_00015148 -->

    <owl:NamedIndividual rdf:about="http://purl.obolibrary.org/obo/GAZ_00015148">
        <rdf:type rdf:resource="http://purl.obolibrary.org/obo/ENVO_00000004"/>
        <obo:RO_0001025 rdf:resource="http://purl.obolibrary.org/obo/GAZ_00009425"/>
        <obo:IAO_0000115>A district of Copperbelt Province.</obo:IAO_0000115>
        <oboInOwl:hasOBONamespace>GAZ</oboInOwl:hasOBONamespace>
        <oboInOwl:id>GAZ:00015148</oboInOwl:id>
        <rdfs:label>Chingola District</rdfs:label>
    </owl:NamedIndividual>
    


    <!-- http://purl.obolibrary.org/obo/GAZ_00015149 -->

    <owl:NamedIndividual rdf:about="http://purl.obolibrary.org/obo/GAZ_00015149">
        <obo:RO_0001025 rdf:resource="http://purl.obolibrary.org/obo/GAZ_00009421"/>
        <obo:IAO_0000115>A District located in the Eastern Province of Zambia.</obo:IAO_0000115>
        <oboInOwl:hasOBONamespace>GAZ</oboInOwl:hasOBONamespace>
        <oboInOwl:id>GAZ:00015149</oboInOwl:id>
        <rdfs:label>Lundazi District</rdfs:label>
    </owl:NamedIndividual>
    


    <!-- http://purl.obolibrary.org/obo/GAZ_00015150 -->

    <owl:NamedIndividual rdf:about="http://purl.obolibrary.org/obo/GAZ_00015150">
        <rdf:type rdf:resource="http://purl.obolibrary.org/obo/ENVO_00000004"/>
        <obo:RO_0001025 rdf:resource="http://purl.obolibrary.org/obo/GAZ_00009425"/>
        <obo:IAO_0000115>A district of Copperbelt Province.</obo:IAO_0000115>
        <oboInOwl:hasOBONamespace>GAZ</oboInOwl:hasOBONamespace>
        <oboInOwl:id>GAZ:00015150</oboInOwl:id>
        <rdfs:label>Masaiti District</rdfs:label>
    </owl:NamedIndividual>
    


    <!-- http://purl.obolibrary.org/obo/GAZ_00015151 -->

    <owl:NamedIndividual rdf:about="http://purl.obolibrary.org/obo/GAZ_00015151">
        <obo:RO_0001025 rdf:resource="http://purl.obolibrary.org/obo/GAZ_00009421"/>
        <obo:IAO_0000115>A District located in the Eastern Province of Zambia.</obo:IAO_0000115>
        <oboInOwl:hasOBONamespace>GAZ</oboInOwl:hasOBONamespace>
        <oboInOwl:id>GAZ:00015151</oboInOwl:id>
        <rdfs:label>Katete District</rdfs:label>
    </owl:NamedIndividual>
    


    <!-- http://purl.obolibrary.org/obo/GAZ_00015152 -->

    <owl:NamedIndividual rdf:about="http://purl.obolibrary.org/obo/GAZ_00015152">
        <obo:RO_0001025 rdf:resource="http://purl.obolibrary.org/obo/GAZ_00009421"/>
        <obo:IAO_0000115>A District located in the Eastern Province of Zambia.</obo:IAO_0000115>
        <oboInOwl:hasOBONamespace>GAZ</oboInOwl:hasOBONamespace>
        <oboInOwl:id>GAZ:00015152</oboInOwl:id>
        <rdfs:label>Mambwe District</rdfs:label>
    </owl:NamedIndividual>
    


    <!-- http://purl.obolibrary.org/obo/GAZ_00015153 -->

    <owl:NamedIndividual rdf:about="http://purl.obolibrary.org/obo/GAZ_00015153">
        <obo:RO_0001025 rdf:resource="http://purl.obolibrary.org/obo/GAZ_00009421"/>
        <obo:IAO_0000115>A District located in the Eastern Province of Zambia.</obo:IAO_0000115>
        <oboInOwl:hasOBONamespace>GAZ</oboInOwl:hasOBONamespace>
        <oboInOwl:id>GAZ:00015153</oboInOwl:id>
        <rdfs:label>Nyimba District</rdfs:label>
    </owl:NamedIndividual>
    


    <!-- http://purl.obolibrary.org/obo/GAZ_00015154 -->

    <owl:NamedIndividual rdf:about="http://purl.obolibrary.org/obo/GAZ_00015154">
        <obo:RO_0001025 rdf:resource="http://purl.obolibrary.org/obo/GAZ_00009421"/>
        <obo:IAO_0000115>A District located in the Eastern Province of Zambia.</obo:IAO_0000115>
        <oboInOwl:hasOBONamespace>GAZ</oboInOwl:hasOBONamespace>
        <oboInOwl:id>GAZ:00015154</oboInOwl:id>
        <rdfs:label>Petauke District</rdfs:label>
    </owl:NamedIndividual>
    


    <!-- http://purl.obolibrary.org/obo/GAZ_00015155 -->

    <owl:NamedIndividual rdf:about="http://purl.obolibrary.org/obo/GAZ_00015155">
        <obo:RO_0001025 rdf:resource="http://purl.obolibrary.org/obo/GAZ_00009421"/>
        <obo:IAO_0000115>The most northerly, largest and least-populated district of the Eastern Province and includes a large wilderness in the Upper Luangwa valley just north-east of the North Luangwa National Park.</obo:IAO_0000115>
        <oboInOwl:hasOBONamespace>GAZ</oboInOwl:hasOBONamespace>
        <oboInOwl:id>GAZ:00015155</oboInOwl:id>
        <rdfs:label>Chama District</rdfs:label>
    </owl:NamedIndividual>
    


    <!-- http://purl.obolibrary.org/obo/GAZ_00015156 -->

    <owl:NamedIndividual rdf:about="http://purl.obolibrary.org/obo/GAZ_00015156">
        <rdf:type rdf:resource="http://purl.obolibrary.org/obo/ENVO_00000004"/>
        <obo:RO_0001025 rdf:resource="http://purl.obolibrary.org/obo/GAZ_00009421"/>
        <obo:IAO_0000115>A district that lies in the extreme south-east corner of Zambia, bordering Malawi to its east and Mozambique to its south.</obo:IAO_0000115>
        <oboInOwl:hasOBONamespace>GAZ</oboInOwl:hasOBONamespace>
        <oboInOwl:id>GAZ:00015156</oboInOwl:id>
        <rdfs:label>Chadiza District</rdfs:label>
    </owl:NamedIndividual>
    


    <!-- http://purl.obolibrary.org/obo/GAZ_00015157 -->

    <owl:NamedIndividual rdf:about="http://purl.obolibrary.org/obo/GAZ_00015157">
        <rdf:type rdf:resource="http://purl.obolibrary.org/obo/ENVO_00000004"/>
        <obo:RO_0001025 rdf:resource="http://purl.obolibrary.org/obo/GAZ_00009427"/>
        <obo:IAO_0000115>A district of Luaplula Province.</obo:IAO_0000115>
        <oboInOwl:hasOBONamespace>GAZ</oboInOwl:hasOBONamespace>
        <oboInOwl:id>GAZ:00015157</oboInOwl:id>
        <rdfs:label>Nchelenge District</rdfs:label>
    </owl:NamedIndividual>
    


    <!-- http://purl.obolibrary.org/obo/GAZ_00015158 -->

    <owl:NamedIndividual rdf:about="http://purl.obolibrary.org/obo/GAZ_00015158">
        <rdf:type rdf:resource="http://purl.obolibrary.org/obo/ENVO_00000004"/>
        <obo:RO_0001025 rdf:resource="http://purl.obolibrary.org/obo/GAZ_00009427"/>
        <obo:IAO_0000115>A district of Luaplula Province.</obo:IAO_0000115>
        <oboInOwl:hasOBONamespace>GAZ</oboInOwl:hasOBONamespace>
        <oboInOwl:id>GAZ:00015158</oboInOwl:id>
        <rdfs:label>Mansa District</rdfs:label>
    </owl:NamedIndividual>
    


    <!-- http://purl.obolibrary.org/obo/GAZ_00015159 -->

    <owl:NamedIndividual rdf:about="http://purl.obolibrary.org/obo/GAZ_00015159">
        <obo:RO_0001025 rdf:resource="http://purl.obolibrary.org/obo/GAZ_00009427"/>
        <obo:IAO_0000115>The smallest and most northerly district in the Luapula Province and was carved out of Nchelenge District after Zambia&apos;s independence.</obo:IAO_0000115>
        <oboInOwl:hasOBONamespace>GAZ</oboInOwl:hasOBONamespace>
        <oboInOwl:id>GAZ:00015159</oboInOwl:id>
        <rdfs:label>Chiengi District</rdfs:label>
    </owl:NamedIndividual>
    


    <!-- http://purl.obolibrary.org/obo/GAZ_00015160 -->

    <owl:NamedIndividual rdf:about="http://purl.obolibrary.org/obo/GAZ_00015160">
        <rdf:type rdf:resource="http://purl.obolibrary.org/obo/ENVO_00000004"/>
        <obo:RO_0001025 rdf:resource="http://purl.obolibrary.org/obo/GAZ_00009427"/>
        <obo:IAO_0000115>A district of Luaplula Province.</obo:IAO_0000115>
        <oboInOwl:hasOBONamespace>GAZ</oboInOwl:hasOBONamespace>
        <oboInOwl:id>GAZ:00015160</oboInOwl:id>
        <rdfs:label>Mwense District</rdfs:label>
    </owl:NamedIndividual>
    


    <!-- http://purl.obolibrary.org/obo/GAZ_00015161 -->

    <owl:NamedIndividual rdf:about="http://purl.obolibrary.org/obo/GAZ_00015161">
        <rdf:type rdf:resource="http://purl.obolibrary.org/obo/ENVO_00000004"/>
        <obo:RO_0001025 rdf:resource="http://purl.obolibrary.org/obo/GAZ_00009427"/>
        <obo:IAO_0000115>A district of Luaplula Province.</obo:IAO_0000115>
        <oboInOwl:hasOBONamespace>GAZ</oboInOwl:hasOBONamespace>
        <oboInOwl:id>GAZ:00015161</oboInOwl:id>
        <rdfs:label>Kawambwa District</rdfs:label>
    </owl:NamedIndividual>
    


    <!-- http://purl.obolibrary.org/obo/GAZ_00015162 -->

    <owl:NamedIndividual rdf:about="http://purl.obolibrary.org/obo/GAZ_00015162">
        <obo:RO_0001025 rdf:resource="http://purl.obolibrary.org/obo/GAZ_00009427"/>
        <obo:IAO_0000115>The most southerly district in the Luapula Province and was carved out of Mansa District. Its southern boundary is the Luapula River which divides it from DR Congo and the district lies roughly between the Chembe Ferry to Mansa road in the west and the Kapalala Ferry to Samfya road in the east.</obo:IAO_0000115>
        <oboInOwl:hasOBONamespace>GAZ</oboInOwl:hasOBONamespace>
        <oboInOwl:id>GAZ:00015162</oboInOwl:id>
        <rdfs:label>Milenge District</rdfs:label>
    </owl:NamedIndividual>
    


    <!-- http://purl.obolibrary.org/obo/GAZ_00015163 -->

    <owl:NamedIndividual rdf:about="http://purl.obolibrary.org/obo/GAZ_00015163">
        <rdf:type rdf:resource="http://purl.obolibrary.org/obo/ENVO_00000004"/>
        <obo:RO_0001025 rdf:resource="http://purl.obolibrary.org/obo/GAZ_00009427"/>
        <obo:IAO_0000115>A district that is mostly lake, swamp and floodplain. It covers Lake Bangweulu and the Bangweulu swamps, except for the north-east corner which lies in Chilubi District of Northern Province. The only extensive dry land is along its western edge where it borders Milenge and Mansa Districts. There are numerous inhabited islands in the lake and swamps, as well as peninsulas almost entirely surrounded by water, such as the Twingi peninsula.</obo:IAO_0000115>
        <oboInOwl:hasOBONamespace>GAZ</oboInOwl:hasOBONamespace>
        <oboInOwl:id>GAZ:00015163</oboInOwl:id>
        <rdfs:label>Samfya District</rdfs:label>
    </owl:NamedIndividual>
    


    <!-- http://purl.obolibrary.org/obo/GAZ_00015164 -->

    <owl:NamedIndividual rdf:about="http://purl.obolibrary.org/obo/GAZ_00015164">
        <rdf:type rdf:resource="http://purl.obolibrary.org/obo/ENVO_00000004"/>
        <obo:RO_0001025 rdf:resource="http://purl.obolibrary.org/obo/GAZ_00009420"/>
        <obo:IAO_0000115>A district of Lusaka Province.</obo:IAO_0000115>
        <oboInOwl:hasOBONamespace>GAZ</oboInOwl:hasOBONamespace>
        <oboInOwl:id>GAZ:00015164</oboInOwl:id>
        <rdfs:label>Chongwe District</rdfs:label>
    </owl:NamedIndividual>
    


    <!-- http://purl.obolibrary.org/obo/GAZ_00015165 -->

    <owl:NamedIndividual rdf:about="http://purl.obolibrary.org/obo/GAZ_00015165">
        <rdf:type rdf:resource="http://purl.obolibrary.org/obo/ENVO_00000004"/>
        <obo:RO_0001025 rdf:resource="http://purl.obolibrary.org/obo/GAZ_00009420"/>
        <obo:IAO_0000115>A district of Lusaka Province.</obo:IAO_0000115>
        <oboInOwl:hasOBONamespace>GAZ</oboInOwl:hasOBONamespace>
        <oboInOwl:id>GAZ:00015165</oboInOwl:id>
        <rdfs:label>Luangwa District</rdfs:label>
    </owl:NamedIndividual>
    


    <!-- http://purl.obolibrary.org/obo/GAZ_00015166 -->

    <owl:NamedIndividual rdf:about="http://purl.obolibrary.org/obo/GAZ_00015166">
        <rdf:type rdf:resource="http://purl.obolibrary.org/obo/ENVO_00000004"/>
        <obo:RO_0001025 rdf:resource="http://purl.obolibrary.org/obo/GAZ_00009420"/>
        <obo:IAO_0000115>A district of Lusaka Province.</obo:IAO_0000115>
        <oboInOwl:hasOBONamespace>GAZ</oboInOwl:hasOBONamespace>
        <oboInOwl:id>GAZ:00015166</oboInOwl:id>
        <rdfs:label>Kafue District</rdfs:label>
    </owl:NamedIndividual>
    


    <!-- http://purl.obolibrary.org/obo/GAZ_00015167 -->

    <owl:NamedIndividual rdf:about="http://purl.obolibrary.org/obo/GAZ_00015167">
        <rdf:type rdf:resource="http://purl.obolibrary.org/obo/ENVO_00000004"/>
        <obo:RO_0001025 rdf:resource="http://purl.obolibrary.org/obo/GAZ_00009428"/>
        <obo:IAO_0000115>A district of North-Western Province.</obo:IAO_0000115>
        <oboInOwl:hasOBONamespace>GAZ</oboInOwl:hasOBONamespace>
        <oboInOwl:id>GAZ:00015167</oboInOwl:id>
        <rdfs:label>Chavuma District</rdfs:label>
    </owl:NamedIndividual>
    


    <!-- http://purl.obolibrary.org/obo/GAZ_00015168 -->

    <owl:NamedIndividual rdf:about="http://purl.obolibrary.org/obo/GAZ_00015168">
        <rdf:type rdf:resource="http://purl.obolibrary.org/obo/ENVO_00000004"/>
        <obo:RO_0001025 rdf:resource="http://purl.obolibrary.org/obo/GAZ_00009428"/>
        <obo:IAO_0000115>A district of North-Western Province.</obo:IAO_0000115>
        <oboInOwl:hasOBONamespace>GAZ</oboInOwl:hasOBONamespace>
        <oboInOwl:id>GAZ:00015168</oboInOwl:id>
        <rdfs:label>Mufumbwe District</rdfs:label>
    </owl:NamedIndividual>
    


    <!-- http://purl.obolibrary.org/obo/GAZ_00015169 -->

    <owl:NamedIndividual rdf:about="http://purl.obolibrary.org/obo/GAZ_00015169">
        <rdf:type rdf:resource="http://purl.obolibrary.org/obo/ENVO_00000004"/>
        <obo:RO_0001025 rdf:resource="http://purl.obolibrary.org/obo/GAZ_00009428"/>
        <obo:IAO_0000115>A district of North-Western Province.</obo:IAO_0000115>
        <oboInOwl:hasOBONamespace>GAZ</oboInOwl:hasOBONamespace>
        <oboInOwl:id>GAZ:00015169</oboInOwl:id>
        <rdfs:label>Solwezi District</rdfs:label>
    </owl:NamedIndividual>
    


    <!-- http://purl.obolibrary.org/obo/GAZ_00015170 -->

    <owl:NamedIndividual rdf:about="http://purl.obolibrary.org/obo/GAZ_00015170">
        <rdf:type rdf:resource="http://purl.obolibrary.org/obo/ENVO_00000004"/>
        <obo:RO_0001025 rdf:resource="http://purl.obolibrary.org/obo/GAZ_00009428"/>
        <obo:IAO_0000115>A district of North-Western Province.</obo:IAO_0000115>
        <oboInOwl:hasOBONamespace>GAZ</oboInOwl:hasOBONamespace>
        <oboInOwl:id>GAZ:00015170</oboInOwl:id>
        <rdfs:label>Kasempa District</rdfs:label>
    </owl:NamedIndividual>
    


    <!-- http://purl.obolibrary.org/obo/GAZ_00015171 -->

    <owl:NamedIndividual rdf:about="http://purl.obolibrary.org/obo/GAZ_00015171">
        <rdf:type rdf:resource="http://purl.obolibrary.org/obo/ENVO_00000004"/>
        <obo:RO_0001025 rdf:resource="http://purl.obolibrary.org/obo/GAZ_00009428"/>
        <obo:IAO_0000115>A district of North-Western Province.</obo:IAO_0000115>
        <oboInOwl:hasOBONamespace>GAZ</oboInOwl:hasOBONamespace>
        <oboInOwl:id>GAZ:00015171</oboInOwl:id>
        <rdfs:label>Kabompo District</rdfs:label>
    </owl:NamedIndividual>
    


    <!-- http://purl.obolibrary.org/obo/GAZ_00015172 -->

    <owl:NamedIndividual rdf:about="http://purl.obolibrary.org/obo/GAZ_00015172">
        <rdf:type rdf:resource="http://purl.obolibrary.org/obo/ENVO_00000004"/>
        <obo:RO_0001025 rdf:resource="http://purl.obolibrary.org/obo/GAZ_00009428"/>
        <obo:IAO_0000115>A district of North-Western Province.</obo:IAO_0000115>
        <oboInOwl:hasOBONamespace>GAZ</oboInOwl:hasOBONamespace>
        <oboInOwl:id>GAZ:00015172</oboInOwl:id>
        <rdfs:label>Mwinilunga District</rdfs:label>
    </owl:NamedIndividual>
    


    <!-- http://purl.obolibrary.org/obo/GAZ_00015173 -->

    <owl:NamedIndividual rdf:about="http://purl.obolibrary.org/obo/GAZ_00015173">
        <rdf:type rdf:resource="http://purl.obolibrary.org/obo/ENVO_00000004"/>
        <obo:RO_0001025 rdf:resource="http://purl.obolibrary.org/obo/GAZ_00009428"/>
        <obo:IAO_0000115>A district of North-Western Province.</obo:IAO_0000115>
        <oboInOwl:hasOBONamespace>GAZ</oboInOwl:hasOBONamespace>
        <oboInOwl:id>GAZ:00015173</oboInOwl:id>
        <rdfs:label>Zambezi District</rdfs:label>
    </owl:NamedIndividual>
    


    <!-- http://purl.obolibrary.org/obo/GAZ_00015174 -->

    <owl:NamedIndividual rdf:about="http://purl.obolibrary.org/obo/GAZ_00015174">
        <rdf:type rdf:resource="http://purl.obolibrary.org/obo/ENVO_00000004"/>
        <obo:RO_0001025 rdf:resource="http://purl.obolibrary.org/obo/GAZ_00009423"/>
        <obo:IAO_0000115>A district of Northern Province.</obo:IAO_0000115>
        <oboInOwl:hasOBONamespace>GAZ</oboInOwl:hasOBONamespace>
        <oboInOwl:id>GAZ:00015174</oboInOwl:id>
        <rdfs:label>Mbala District</rdfs:label>
    </owl:NamedIndividual>
    


    <!-- http://purl.obolibrary.org/obo/GAZ_00015175 -->

    <owl:NamedIndividual rdf:about="http://purl.obolibrary.org/obo/GAZ_00015175">
        <rdf:type rdf:resource="http://purl.obolibrary.org/obo/ENVO_00000004"/>
        <obo:RO_0001025 rdf:resource="http://purl.obolibrary.org/obo/GAZ_00009423"/>
        <obo:IAO_0000115>A district of Northern Province.</obo:IAO_0000115>
        <oboInOwl:hasOBONamespace>GAZ</oboInOwl:hasOBONamespace>
        <oboInOwl:id>GAZ:00015175</oboInOwl:id>
        <rdfs:label>Mpika District</rdfs:label>
    </owl:NamedIndividual>
    


    <!-- http://purl.obolibrary.org/obo/GAZ_00015176 -->

    <owl:NamedIndividual rdf:about="http://purl.obolibrary.org/obo/GAZ_00015176">
        <rdf:type rdf:resource="http://purl.obolibrary.org/obo/ENVO_00000004"/>
        <obo:RO_0001025 rdf:resource="http://purl.obolibrary.org/obo/GAZ_00009423"/>
        <obo:IAO_0000115>A district of Northern Province.</obo:IAO_0000115>
        <oboInOwl:hasOBONamespace>GAZ</oboInOwl:hasOBONamespace>
        <oboInOwl:id>GAZ:00015176</oboInOwl:id>
        <rdfs:label>Kaputa District</rdfs:label>
    </owl:NamedIndividual>
    


    <!-- http://purl.obolibrary.org/obo/GAZ_00015177 -->

    <owl:NamedIndividual rdf:about="http://purl.obolibrary.org/obo/GAZ_00015177">
        <rdf:type rdf:resource="http://purl.obolibrary.org/obo/ENVO_00000004"/>
        <obo:RO_0001025 rdf:resource="http://purl.obolibrary.org/obo/GAZ_00009423"/>
        <obo:IAO_0000115>A district of Northern Province.</obo:IAO_0000115>
        <oboInOwl:hasOBONamespace>GAZ</oboInOwl:hasOBONamespace>
        <oboInOwl:id>GAZ:00015177</oboInOwl:id>
        <rdfs:label>Mpulungu District</rdfs:label>
    </owl:NamedIndividual>
    


    <!-- http://purl.obolibrary.org/obo/GAZ_00015178 -->

    <owl:NamedIndividual rdf:about="http://purl.obolibrary.org/obo/GAZ_00015178">
        <obo:RO_0001025 rdf:resource="http://purl.obolibrary.org/obo/GAZ_00009423"/>
        <obo:IAO_0000115>A central district of Northern Province, Zambia. It surrounds the provincial capital of Kasama town.</obo:IAO_0000115>
        <oboInOwl:hasOBONamespace>GAZ</oboInOwl:hasOBONamespace>
        <oboInOwl:id>GAZ:00015178</oboInOwl:id>
        <rdfs:label>Kasama District</rdfs:label>
    </owl:NamedIndividual>
    


    <!-- http://purl.obolibrary.org/obo/GAZ_00015179 -->

    <owl:NamedIndividual rdf:about="http://purl.obolibrary.org/obo/GAZ_00015179">
        <rdf:type rdf:resource="http://purl.obolibrary.org/obo/ENVO_00000004"/>
        <obo:RO_0001025 rdf:resource="http://purl.obolibrary.org/obo/GAZ_00009423"/>
        <obo:IAO_0000115>A district of Northern Province.</obo:IAO_0000115>
        <oboInOwl:hasOBONamespace>GAZ</oboInOwl:hasOBONamespace>
        <oboInOwl:id>GAZ:00015179</oboInOwl:id>
        <rdfs:label>Mungwi District</rdfs:label>
    </owl:NamedIndividual>
    


    <!-- http://purl.obolibrary.org/obo/GAZ_00015180 -->

    <owl:NamedIndividual rdf:about="http://purl.obolibrary.org/obo/GAZ_00015180">
        <rdf:type rdf:resource="http://purl.obolibrary.org/obo/ENVO_00000004"/>
        <obo:RO_0001025 rdf:resource="http://purl.obolibrary.org/obo/GAZ_00009423"/>
        <obo:IAO_0000115>A district that lies on the watershed between the Chambeshi River in the Congo basin and the Luangwa River in the Zambezi basin.</obo:IAO_0000115>
        <oboInOwl:hasOBONamespace>GAZ</oboInOwl:hasOBONamespace>
        <oboInOwl:id>GAZ:00015180</oboInOwl:id>
        <rdfs:label>Chinsali District</rdfs:label>
    </owl:NamedIndividual>
    


    <!-- http://purl.obolibrary.org/obo/GAZ_00015181 -->

    <owl:NamedIndividual rdf:about="http://purl.obolibrary.org/obo/GAZ_00015181">
        <rdf:type rdf:resource="http://purl.obolibrary.org/obo/ENVO_00000004"/>
        <obo:RO_0001025 rdf:resource="http://purl.obolibrary.org/obo/GAZ_00009423"/>
        <obo:IAO_0000115>A district of Northern Province.</obo:IAO_0000115>
        <oboInOwl:hasOBONamespace>GAZ</oboInOwl:hasOBONamespace>
        <oboInOwl:id>GAZ:00015181</oboInOwl:id>
        <rdfs:label>Mporokoso District</rdfs:label>
    </owl:NamedIndividual>
    


    <!-- http://purl.obolibrary.org/obo/GAZ_00015182 -->

    <owl:NamedIndividual rdf:about="http://purl.obolibrary.org/obo/GAZ_00015182">
        <rdf:type rdf:resource="http://purl.obolibrary.org/obo/ENVO_00000004"/>
        <obo:RO_0001025 rdf:resource="http://purl.obolibrary.org/obo/GAZ_00009423"/>
        <obo:IAO_0000115>A district of Northern Province that covers the north-east Lake Bangweulu and Bangweulu swamps containing several islands including Chilubi Island, and some of the mainland northeast of the lake.</obo:IAO_0000115>
        <oboInOwl:hasOBONamespace>GAZ</oboInOwl:hasOBONamespace>
        <oboInOwl:id>GAZ:00015182</oboInOwl:id>
        <rdfs:label>Chilubi District</rdfs:label>
    </owl:NamedIndividual>
    


    <!-- http://purl.obolibrary.org/obo/GAZ_00015183 -->

    <owl:NamedIndividual rdf:about="http://purl.obolibrary.org/obo/GAZ_00015183">
        <rdf:type rdf:resource="http://purl.obolibrary.org/obo/ENVO_00000004"/>
        <obo:RO_0001025 rdf:resource="http://purl.obolibrary.org/obo/GAZ_00009423"/>
        <obo:IAO_0000115>A district of Northern Province.</obo:IAO_0000115>
        <oboInOwl:hasOBONamespace>GAZ</oboInOwl:hasOBONamespace>
        <oboInOwl:id>GAZ:00015183</oboInOwl:id>
        <rdfs:label>Isoka District</rdfs:label>
    </owl:NamedIndividual>
    


    <!-- http://purl.obolibrary.org/obo/GAZ_00015184 -->

    <owl:NamedIndividual rdf:about="http://purl.obolibrary.org/obo/GAZ_00015184">
        <rdf:type rdf:resource="http://purl.obolibrary.org/obo/ENVO_00000004"/>
        <obo:RO_0001025 rdf:resource="http://purl.obolibrary.org/obo/GAZ_00009423"/>
        <obo:IAO_0000115>A district of Northern Province.</obo:IAO_0000115>
        <oboInOwl:hasOBONamespace>GAZ</oboInOwl:hasOBONamespace>
        <oboInOwl:id>GAZ:00015184</oboInOwl:id>
        <rdfs:label>Luwingu District</rdfs:label>
    </owl:NamedIndividual>
    


    <!-- http://purl.obolibrary.org/obo/GAZ_00015185 -->

    <owl:NamedIndividual rdf:about="http://purl.obolibrary.org/obo/GAZ_00015185">
        <rdf:type rdf:resource="http://purl.obolibrary.org/obo/ENVO_00000004"/>
        <obo:RO_0001025 rdf:resource="http://purl.obolibrary.org/obo/GAZ_00009423"/>
        <obo:IAO_0000115>A district of Northern Province.</obo:IAO_0000115>
        <oboInOwl:hasOBONamespace>GAZ</oboInOwl:hasOBONamespace>
        <oboInOwl:id>GAZ:00015185</oboInOwl:id>
        <rdfs:label>Nakonde District</rdfs:label>
    </owl:NamedIndividual>
    


    <!-- http://purl.obolibrary.org/obo/GAZ_00015186 -->

    <owl:NamedIndividual rdf:about="http://purl.obolibrary.org/obo/GAZ_00015186">
        <rdf:type rdf:resource="http://purl.obolibrary.org/obo/ENVO_00000004"/>
        <obo:RO_0001025 rdf:resource="http://purl.obolibrary.org/obo/GAZ_00009422"/>
        <obo:IAO_0000115>A district of Southern Province of Zambia.</obo:IAO_0000115>
        <oboInOwl:hasOBONamespace>GAZ</oboInOwl:hasOBONamespace>
        <oboInOwl:id>GAZ:00015186</oboInOwl:id>
        <rdfs:label>Sinazongwe District</rdfs:label>
    </owl:NamedIndividual>
    


    <!-- http://purl.obolibrary.org/obo/GAZ_00015187 -->

    <owl:NamedIndividual rdf:about="http://purl.obolibrary.org/obo/GAZ_00015187">
        <rdf:type rdf:resource="http://purl.obolibrary.org/obo/ENVO_00000004"/>
        <obo:RO_0001025 rdf:resource="http://purl.obolibrary.org/obo/GAZ_00009422"/>
        <obo:IAO_0000115>A district of Southern Province of Zambia.</obo:IAO_0000115>
        <oboInOwl:hasOBONamespace>GAZ</oboInOwl:hasOBONamespace>
        <oboInOwl:id>GAZ:00015187</oboInOwl:id>
        <rdfs:label>Livingstone District</rdfs:label>
    </owl:NamedIndividual>
    


    <!-- http://purl.obolibrary.org/obo/GAZ_00015188 -->

    <owl:NamedIndividual rdf:about="http://purl.obolibrary.org/obo/GAZ_00015188">
        <rdf:type rdf:resource="http://purl.obolibrary.org/obo/ENVO_00000004"/>
        <obo:RO_0001025 rdf:resource="http://purl.obolibrary.org/obo/GAZ_00009422"/>
        <obo:IAO_0000115>A district of Southern Province of Zambia.</obo:IAO_0000115>
        <oboInOwl:hasOBONamespace>GAZ</oboInOwl:hasOBONamespace>
        <oboInOwl:id>GAZ:00015188</oboInOwl:id>
        <rdfs:label>Siavonga District</rdfs:label>
    </owl:NamedIndividual>
    


    <!-- http://purl.obolibrary.org/obo/GAZ_00015189 -->

    <owl:NamedIndividual rdf:about="http://purl.obolibrary.org/obo/GAZ_00015189">
        <rdf:type rdf:resource="http://purl.obolibrary.org/obo/ENVO_00000004"/>
        <obo:RO_0001025 rdf:resource="http://purl.obolibrary.org/obo/GAZ_00009422"/>
        <obo:IAO_0000115>A district of Southern Province of Zambia.</obo:IAO_0000115>
        <oboInOwl:hasOBONamespace>GAZ</oboInOwl:hasOBONamespace>
        <oboInOwl:id>GAZ:00015189</oboInOwl:id>
        <rdfs:label>Namwala District</rdfs:label>
    </owl:NamedIndividual>
    


    <!-- http://purl.obolibrary.org/obo/GAZ_00015190 -->

    <owl:NamedIndividual rdf:about="http://purl.obolibrary.org/obo/GAZ_00015190">
        <rdf:type rdf:resource="http://purl.obolibrary.org/obo/ENVO_00000004"/>
        <obo:RO_0001025 rdf:resource="http://purl.obolibrary.org/obo/GAZ_00009422"/>
        <obo:IAO_0000115>A district of Southern Province of Zambia.</obo:IAO_0000115>
        <oboInOwl:hasOBONamespace>GAZ</oboInOwl:hasOBONamespace>
        <oboInOwl:id>GAZ:00015190</oboInOwl:id>
        <rdfs:label>Kalomo District</rdfs:label>
    </owl:NamedIndividual>
    


    <!-- http://purl.obolibrary.org/obo/GAZ_00015191 -->

    <owl:NamedIndividual rdf:about="http://purl.obolibrary.org/obo/GAZ_00015191">
        <rdf:type rdf:resource="http://purl.obolibrary.org/obo/ENVO_00000004"/>
        <obo:RO_0001025 rdf:resource="http://purl.obolibrary.org/obo/GAZ_00009422"/>
        <obo:IAO_0000115>A district of Southern Province of Zambia.</obo:IAO_0000115>
        <oboInOwl:hasOBONamespace>GAZ</oboInOwl:hasOBONamespace>
        <oboInOwl:id>GAZ:00015191</oboInOwl:id>
        <rdfs:label>Monze District</rdfs:label>
    </owl:NamedIndividual>
    


    <!-- http://purl.obolibrary.org/obo/GAZ_00015192 -->

    <owl:NamedIndividual rdf:about="http://purl.obolibrary.org/obo/GAZ_00015192">
        <rdf:type rdf:resource="http://purl.obolibrary.org/obo/ENVO_00000004"/>
        <obo:RO_0001025 rdf:resource="http://purl.obolibrary.org/obo/GAZ_00009422"/>
        <obo:IAO_0000115>A district of Southern Province of Zambia.</obo:IAO_0000115>
        <oboInOwl:hasOBONamespace>GAZ</oboInOwl:hasOBONamespace>
        <oboInOwl:id>GAZ:00015192</oboInOwl:id>
        <rdfs:label>Gwembe District</rdfs:label>
    </owl:NamedIndividual>
    


    <!-- http://purl.obolibrary.org/obo/GAZ_00015193 -->

    <owl:NamedIndividual rdf:about="http://purl.obolibrary.org/obo/GAZ_00015193">
        <rdf:type rdf:resource="http://purl.obolibrary.org/obo/ENVO_00000004"/>
        <obo:RO_0001025 rdf:resource="http://purl.obolibrary.org/obo/GAZ_00009422"/>
        <obo:IAO_0000115>A district of Southern Province of Zambia.</obo:IAO_0000115>
        <oboInOwl:hasOBONamespace>GAZ</oboInOwl:hasOBONamespace>
        <oboInOwl:id>GAZ:00015193</oboInOwl:id>
        <rdfs:label>Itezhi-Tezhi District</rdfs:label>
    </owl:NamedIndividual>
    


    <!-- http://purl.obolibrary.org/obo/GAZ_00015194 -->

    <owl:NamedIndividual rdf:about="http://purl.obolibrary.org/obo/GAZ_00015194">
        <rdf:type rdf:resource="http://purl.obolibrary.org/obo/ENVO_00000004"/>
        <obo:RO_0001025 rdf:resource="http://purl.obolibrary.org/obo/GAZ_00009422"/>
        <obo:IAO_0000115>A district of Southern Province of Zambia.</obo:IAO_0000115>
        <oboInOwl:hasOBONamespace>GAZ</oboInOwl:hasOBONamespace>
        <oboInOwl:id>GAZ:00015194</oboInOwl:id>
        <rdfs:label>Mazabuka District</rdfs:label>
    </owl:NamedIndividual>
    


    <!-- http://purl.obolibrary.org/obo/GAZ_00015195 -->

    <owl:NamedIndividual rdf:about="http://purl.obolibrary.org/obo/GAZ_00015195">
        <rdf:type rdf:resource="http://purl.obolibrary.org/obo/ENVO_00000004"/>
        <obo:RO_0001025 rdf:resource="http://purl.obolibrary.org/obo/GAZ_00009422"/>
        <obo:IAO_0000115>A district of Southern Province of Zambia.</obo:IAO_0000115>
        <oboInOwl:hasOBONamespace>GAZ</oboInOwl:hasOBONamespace>
        <oboInOwl:id>GAZ:00015195</oboInOwl:id>
        <rdfs:label>Choma District</rdfs:label>
    </owl:NamedIndividual>
    


    <!-- http://purl.obolibrary.org/obo/GAZ_00015196 -->

    <owl:NamedIndividual rdf:about="http://purl.obolibrary.org/obo/GAZ_00015196">
        <rdf:type rdf:resource="http://purl.obolibrary.org/obo/ENVO_00000004"/>
        <obo:RO_0001025 rdf:resource="http://purl.obolibrary.org/obo/GAZ_00009422"/>
        <obo:IAO_0000115>A district of Southern Province of Zambia.</obo:IAO_0000115>
        <oboInOwl:hasOBONamespace>GAZ</oboInOwl:hasOBONamespace>
        <oboInOwl:id>GAZ:00015196</oboInOwl:id>
        <rdfs:label>Kazungula District</rdfs:label>
    </owl:NamedIndividual>
    


    <!-- http://purl.obolibrary.org/obo/GAZ_00015197 -->

    <owl:NamedIndividual rdf:about="http://purl.obolibrary.org/obo/GAZ_00015197">
        <rdf:type rdf:resource="http://purl.obolibrary.org/obo/ENVO_00000004"/>
        <obo:RO_0001025 rdf:resource="http://purl.obolibrary.org/obo/GAZ_00009430"/>
        <obo:IAO_0000115>A district of Western Province.</obo:IAO_0000115>
        <oboInOwl:hasOBONamespace>GAZ</oboInOwl:hasOBONamespace>
        <oboInOwl:id>GAZ:00015197</oboInOwl:id>
        <rdfs:label>Kalabo District</rdfs:label>
    </owl:NamedIndividual>
    


    <!-- http://purl.obolibrary.org/obo/GAZ_00015198 -->

    <owl:NamedIndividual rdf:about="http://purl.obolibrary.org/obo/GAZ_00015198">
        <rdf:type rdf:resource="http://purl.obolibrary.org/obo/ENVO_00000004"/>
        <obo:RO_0001025 rdf:resource="http://purl.obolibrary.org/obo/GAZ_00009430"/>
        <obo:IAO_0000115>A district of Western Province.</obo:IAO_0000115>
        <oboInOwl:hasOBONamespace>GAZ</oboInOwl:hasOBONamespace>
        <oboInOwl:id>GAZ:00015198</oboInOwl:id>
        <rdfs:label>Shangombo District</rdfs:label>
    </owl:NamedIndividual>
    


    <!-- http://purl.obolibrary.org/obo/GAZ_00015199 -->

    <owl:NamedIndividual rdf:about="http://purl.obolibrary.org/obo/GAZ_00015199">
        <rdf:type rdf:resource="http://purl.obolibrary.org/obo/ENVO_00000004"/>
        <obo:RO_0001025 rdf:resource="http://purl.obolibrary.org/obo/GAZ_00009430"/>
        <obo:IAO_0000115>A district in the north-east corner of Western Province.</obo:IAO_0000115>
        <oboInOwl:hasOBONamespace>GAZ</oboInOwl:hasOBONamespace>
        <oboInOwl:id>GAZ:00015199</oboInOwl:id>
        <rdfs:label>Kaoma District</rdfs:label>
    </owl:NamedIndividual>
    


    <!-- http://purl.obolibrary.org/obo/GAZ_00015200 -->

    <owl:NamedIndividual rdf:about="http://purl.obolibrary.org/obo/GAZ_00015200">
        <rdf:type rdf:resource="http://purl.obolibrary.org/obo/ENVO_00000004"/>
        <obo:RO_0001025 rdf:resource="http://purl.obolibrary.org/obo/GAZ_00009430"/>
        <obo:IAO_0000115>A district of Western Province.</obo:IAO_0000115>
        <oboInOwl:hasOBONamespace>GAZ</oboInOwl:hasOBONamespace>
        <oboInOwl:id>GAZ:00015200</oboInOwl:id>
        <rdfs:label>Sesheke District</rdfs:label>
    </owl:NamedIndividual>
    


    <!-- http://purl.obolibrary.org/obo/GAZ_00015201 -->

    <owl:NamedIndividual rdf:about="http://purl.obolibrary.org/obo/GAZ_00015201">
        <rdf:type rdf:resource="http://purl.obolibrary.org/obo/ENVO_00000004"/>
        <obo:RO_0001025 rdf:resource="http://purl.obolibrary.org/obo/GAZ_00009430"/>
        <obo:IAO_0000115>A district that stretches across the north-eastern and north-central parts of Western Province, adjoining North-Western Province and straddling the Zambezi and the northern Barotse Floodplain.</obo:IAO_0000115>
        <oboInOwl:hasOBONamespace>GAZ</oboInOwl:hasOBONamespace>
        <oboInOwl:id>GAZ:00015201</oboInOwl:id>
        <rdfs:label>Lukulu District</rdfs:label>
    </owl:NamedIndividual>
    


    <!-- http://purl.obolibrary.org/obo/GAZ_00015202 -->

    <owl:NamedIndividual rdf:about="http://purl.obolibrary.org/obo/GAZ_00015202">
        <rdf:type rdf:resource="http://purl.obolibrary.org/obo/ENVO_00000004"/>
        <obo:RO_0001025 rdf:resource="http://purl.obolibrary.org/obo/GAZ_00009430"/>
        <obo:IAO_0000115>A district of Western Province.</obo:IAO_0000115>
        <oboInOwl:hasOBONamespace>GAZ</oboInOwl:hasOBONamespace>
        <oboInOwl:id>GAZ:00015202</oboInOwl:id>
        <rdfs:label>Senanga District</rdfs:label>
    </owl:NamedIndividual>
    


    <!-- http://purl.obolibrary.org/obo/GAZ_00016177 -->

    <owl:NamedIndividual rdf:about="http://purl.obolibrary.org/obo/GAZ_00016177">
        <obo:IAO_0000115>A lake southwest of Harare, Zimbabwe. The lake was created and opened to the public in 1952.</obo:IAO_0000115>
        <oboInOwl:hasOBONamespace>GAZ</oboInOwl:hasOBONamespace>
        <oboInOwl:id>GAZ:00016177</oboInOwl:id>
        <rdfs:label>Lake Chivero</rdfs:label>
    </owl:NamedIndividual>
    


    <!-- http://purl.obolibrary.org/obo/GAZ_00016178 -->

    <owl:NamedIndividual rdf:about="http://purl.obolibrary.org/obo/GAZ_00016178">
        <obo:RO_0001025 rdf:resource="http://purl.obolibrary.org/obo/GAZ_00044898"/>
        <obo:IAO_0000115>A large, artificial lake and reservoir located on the Zambezi river, about halfway between the river&apos;s source and mouth, about 1300 km upstream from the Indian Ocean. The lake lies along the border between Zambia and Zimbabwe.</obo:IAO_0000115>
        <oboInOwl:hasOBONamespace>GAZ</oboInOwl:hasOBONamespace>
        <oboInOwl:id>GAZ:00016178</oboInOwl:id>
        <rdfs:label>Lake Kariba</rdfs:label>
    </owl:NamedIndividual>
    


    <!-- http://purl.obolibrary.org/obo/GAZ_00039986 -->

    <owl:NamedIndividual rdf:about="http://purl.obolibrary.org/obo/GAZ_00039986">
        <obo:RO_0001025 rdf:resource="http://purl.obolibrary.org/obo/GAZ_00044898"/>
        <obo:IAO_0000115>An island that lies where the Chobe River flows into the Zambezi River, forming the easternmost point of Namibia. It neighbours Zambia, Botswana and Zimbabwe.</obo:IAO_0000115>
        <oboInOwl:hasOBONamespace>GAZ</oboInOwl:hasOBONamespace>
        <oboInOwl:id>GAZ:00039986</oboInOwl:id>
        <rdfs:label>Mpalila Island</rdfs:label>
    </owl:NamedIndividual>
    


    <!-- http://purl.obolibrary.org/obo/GAZ_00041529 -->

    <owl:NamedIndividual rdf:about="http://purl.obolibrary.org/obo/GAZ_00041529">
        <obo:IAO_0000115>A lake in southern part of Malawi, in the Southern Region.</obo:IAO_0000115>
        <oboInOwl:hasOBONamespace>GAZ</oboInOwl:hasOBONamespace>
        <oboInOwl:id>GAZ:00041529</oboInOwl:id>
        <rdfs:label>Lake Malombe</rdfs:label>
    </owl:NamedIndividual>
    


    <!-- http://purl.obolibrary.org/obo/GAZ_00041530 -->

    <owl:NamedIndividual rdf:about="http://purl.obolibrary.org/obo/GAZ_00041530">
        <obo:IAO_0000115>A freshwater lake on the longest arm of Africa&apos;s second-longest river, the Congo. Located on the border between Zambia and Democratic Republic of the Congo, it makes up 110 km of the total length of the Congo, lying between its Luapula River (upstream) and Luvua River (downstream) segments. Mweru is mainly fed by the Luapula River, which comes in through swamps from the south, and the Kalungwishi River from the east. At its north end the lake is drained by the Luvua River, which flows in a northwesterly direction to join the Lualaba River and thence to the Congo.</obo:IAO_0000115>
        <oboInOwl:hasOBONamespace>GAZ</oboInOwl:hasOBONamespace>
        <oboInOwl:id>GAZ:00041530</oboInOwl:id>
        <rdfs:label>Lake Mweru</rdfs:label>
    </owl:NamedIndividual>
    


    <!-- http://purl.obolibrary.org/obo/GAZ_00041532 -->

    <owl:NamedIndividual rdf:about="http://purl.obolibrary.org/obo/GAZ_00041532">
        <obo:RO_0001025 rdf:resource="http://purl.obolibrary.org/obo/GAZ_00076746"/>
        <obo:IAO_0000115>An endorheic lake and swamp system in the Northern Province of Zambia. A rift valley lake lying in a branch of the Great Rift Valley, running from the Luapula River to Lake Tanganyika. There are some hot springs characteristics of a rift valley to the east. Its water is muddy in appearance, at times appearing reddish and &apos;slightly oily&apos;.</obo:IAO_0000115>
        <oboInOwl:hasOBONamespace>GAZ</oboInOwl:hasOBONamespace>
        <oboInOwl:id>GAZ:00041532</oboInOwl:id>
        <rdfs:label>Lake Mweru Wantipa</rdfs:label>
    </owl:NamedIndividual>
    


    <!-- http://purl.obolibrary.org/obo/GAZ_00041545 -->

    <owl:NamedIndividual rdf:about="http://purl.obolibrary.org/obo/GAZ_00041545">
        <obo:RO_0001025 rdf:resource="http://purl.obolibrary.org/obo/GAZ_00041530"/>
        <obo:IAO_0000115>An island in Lake Mweru.</obo:IAO_0000115>
        <oboInOwl:hasOBONamespace>GAZ</oboInOwl:hasOBONamespace>
        <oboInOwl:id>GAZ:00041545</oboInOwl:id>
        <rdfs:label>Kilwa Island</rdfs:label>
    </owl:NamedIndividual>
    


    <!-- http://purl.obolibrary.org/obo/GAZ_00041546 -->

    <owl:NamedIndividual rdf:about="http://purl.obolibrary.org/obo/GAZ_00041546">
        <obo:RO_0001025 rdf:resource="http://purl.obolibrary.org/obo/GAZ_00041530"/>
        <oboInOwl:hasOBONamespace>GAZ</oboInOwl:hasOBONamespace>
        <oboInOwl:id>GAZ:00041546</oboInOwl:id>
        <rdfs:label>Isokwe Island</rdfs:label>
    </owl:NamedIndividual>
    


    <!-- http://purl.obolibrary.org/obo/GAZ_00044898 -->

    <owl:NamedIndividual rdf:about="http://purl.obolibrary.org/obo/GAZ_00044898">
        <obo:IAO_0000115>A river that rises in a black marshy dambo in north-western Zambia, in undulating miombo woodland, quite dense in parts, about 1,500 m above sea level. Eastward of the source the watershed between the Congo and Zambezi basins is a well-marked belt of high ground, falling abruptly north and south, and running nearly east-west. This distinctly cuts off the basin of the Lualaba (the main branch of the upper Congo) from that of the Zambezi. In the neighborhood of the source the watershed is not as clearly defined, but the two river systems do not connect. The river flows to the south-west and into Angola for about 240 km, then is joined by sizeable tributaries such as the Luena and the Chifumage flowing from highlands to the north-west. It turns south and develops a floodplain and becomes very variable in width between the dry and rainy seasons. It enters a region with dense patches of evergreen Cryptosepalum dry forest, though on its wesern side, Western Zambezian grasslands also occur. Where it re-enters Zambia it is nearly 400 m wide in the rainy season and flows quite quickly with rapids ending in the Chavuma Falls, where the river flows through a rocky fissure. The river drops about 400 m in elevation from its source to the at 1500 m to the Chavuma Falls at 1100 metres, in a distance of about 400 km. From this point to the Victoria Falls, the level of the basin is very uniform, dropping only by another 180 m in a distance of around 800 km. The first of its large tributaries to enter the Zambezi is the Kabompo River in the north-western province of Zambia. The savanna through which the river has flowed gives way to a wide floodplain, studded with Borassus fan palms. A little farther south is the confluence with the Lungwebungu River. This is the beginning of the Barotse Floodplain, the most notable feature of the upper Zambezi, but this northern part does not flood so much and includes islands of higher land in the middle. Thirty km below the confluence of the Lungwebungu the country becomes very flat, and the typical Barotse Floodplain landscape unfolds, with the flood reaching a width of 25 km in the rainy season. For more than 200 km downstream the annual flood cycle dominates the natural environment and human life, society and culture. Eighty km further down, the Luanginga, which with its tributaries drains a large area to the west, joins the Zambezi. A few km higher up on the east the main stream is joined in the rainy season by overflow of the Luampa/Luena system. The Victoria Falls are considered the boundary between the upper and middle Zambezi. Below them the river continues to flow due east for about 200 km, cutting through perpendicular walls of basalt 20 to 60 m apart in hills 200 to 250 m high. The river flows swiftly through the gorge, the current being continually interrupted by reefs. Beyond the gorge are a succession of rapids which end 240 km below Victoria Falls. Over this distance, the river drops 250 m. At this point, the river enters Lake Kariba, created in 1959 following the completion of the Kariba Dam. The lake is one of the largest artificial lakes in the world, and the hydroelectric power-generating facilities at the dam provide electricity to much of Zambia and Zimbabwe. The Luangwa and the Kafue are the two largest left-hand tributaries of the Zambezi. The Kafue joins the main river in a quiet deep stream about 180 m wide. From this point the northward bend of the Zambezi is checked and the stream continues due east. At the confluence of the Luangwa it enters Mozambique. The middle Zambezi ends when the river enters Lake Cahora Bassa (also spelled Cabora Bassa). Formerly the site of dangerous rapids known as Kebrabassa, the lake was created in 1974 by the construction of the Cahora Bassa Dam. The lower Zambezi&apos;s 650 km from Cahora Bassa to the Indian Ocean is navigable, although the river is shallow in many places during the dry season. This shallowness arises as the river enters a broad valley and spreads out over a large area. Only at one point, the Lupata Gorge, 320 km from its mouth, is the river confined between high hills. Here it is scarcely 200 m wide. Elsewhere it is from 5 to 8 km wide, flowing gently in many streams. The river bed is sandy, and the banks are low and reed-fringed. At places, however, and especially in the rainy season, the streams unite into one broad fast-flowing river. About 160 km from the sea the Zambezi receives the drainage of Lake Malawi through the Shire River. On approaching the Indian Ocean, the river splits up into a number of branches and forms a wide delta. Each of the four principal mouths, Milambe, Kongone, Luabo and Timbwe, is obstructed by a sand bar. A more northerly branch, called the Chinde mouth, has a minimum depth at low water of 2 m at the entrance and 4 m further in, and is the branch used for navigation. 100 km further north is a river called the Quelimane, after the town at its mouth. This stream, which is silting up, receives the overflow of the Zambezi in the rainy season. The delta of the Zambezi is today about half as broad as it was before the construction of the Kariba and Cahora Bassa dams controlled the seasonal variations in the flow rate of the river. A short distance downstream of the confluence with the Luanginga is Lealui, after which, the river turns to south-south-east. From the east it continues to receive numerous small streams, but on the west is without major tributaries for 240 km. Before this, the Ngonye Falls and subsequent rapids interrupt navigation. South of Ngonye Falls, the river briefly borders Namibia&apos;s Caprivi Strip. The strip projects from the main body of Namibia, and results from the colonial era: it was added to German South-West Africa expressly to give Germany access to the Zambezi. Below the junction of the Cuando River and the Zambezi the river bends almost due east. Here, the river is very broad and shallow, and flows fairly slowly, but as it flows eastward towards the border of the great central plateau of Africa it reaches a chasm into which the Victoria Falls plunge.</obo:IAO_0000115>
        <oboInOwl:hasOBONamespace>GAZ</oboInOwl:hasOBONamespace>
        <oboInOwl:id>GAZ:00044898</oboInOwl:id>
        <rdfs:label>Zambezi River</rdfs:label>
    </owl:NamedIndividual>
    


    <!-- http://purl.obolibrary.org/obo/GAZ_00044899 -->

    <owl:NamedIndividual rdf:about="http://purl.obolibrary.org/obo/GAZ_00044899">
        <obo:RO_0001025 rdf:resource="http://purl.obolibrary.org/obo/GAZ_00016178"/>
        <obo:IAO_0000115>An island of Lake Kariba.</obo:IAO_0000115>
        <oboInOwl:hasOBONamespace>GAZ</oboInOwl:hasOBONamespace>
        <oboInOwl:id>GAZ:00044899</oboInOwl:id>
        <rdfs:label>Chete Island</rdfs:label>
    </owl:NamedIndividual>
    


    <!-- http://purl.obolibrary.org/obo/GAZ_00044900 -->

    <owl:NamedIndividual rdf:about="http://purl.obolibrary.org/obo/GAZ_00044900">
        <obo:RO_0001025 rdf:resource="http://purl.obolibrary.org/obo/GAZ_00016178"/>
        <obo:IAO_0000115>An island of Lake Kariba.</obo:IAO_0000115>
        <oboInOwl:hasOBONamespace>GAZ</oboInOwl:hasOBONamespace>
        <oboInOwl:id>GAZ:00044900</oboInOwl:id>
        <rdfs:label>Sekula Island</rdfs:label>
    </owl:NamedIndividual>
    


    <!-- http://purl.obolibrary.org/obo/GAZ_00044901 -->

    <owl:NamedIndividual rdf:about="http://purl.obolibrary.org/obo/GAZ_00044901">
        <obo:RO_0001025 rdf:resource="http://purl.obolibrary.org/obo/GAZ_00016178"/>
        <obo:IAO_0000115>An island of Lake Kariba.</obo:IAO_0000115>
        <oboInOwl:hasOBONamespace>GAZ</oboInOwl:hasOBONamespace>
        <oboInOwl:id>GAZ:00044901</oboInOwl:id>
        <rdfs:label>Chikanka Island</rdfs:label>
    </owl:NamedIndividual>
    


    <!-- http://purl.obolibrary.org/obo/GAZ_00044913 -->

    <owl:NamedIndividual rdf:about="http://purl.obolibrary.org/obo/GAZ_00044913">
        <obo:RO_0001025 rdf:resource="http://purl.obolibrary.org/obo/GAZ_00044898"/>
        <obo:IAO_0000115>An artificial lake, being an impoundment of the middle Zambezi River. Constructed 1966-1975.</obo:IAO_0000115>
        <oboInOwl:hasOBONamespace>GAZ</oboInOwl:hasOBONamespace>
        <oboInOwl:id>GAZ:00044913</oboInOwl:id>
        <rdfs:label>Cahora Bassa</rdfs:label>
    </owl:NamedIndividual>
    


    <!-- http://purl.obolibrary.org/obo/GAZ_00049226 -->

    <owl:NamedIndividual rdf:about="http://purl.obolibrary.org/obo/GAZ_00049226">
        <obo:IAO_0000115>A lake in the upper Congo River basin in Luapula Province, Zambia.</obo:IAO_0000115>
        <oboInOwl:hasOBONamespace>GAZ</oboInOwl:hasOBONamespace>
        <oboInOwl:id>GAZ:00049226</oboInOwl:id>
        <rdfs:label>Lake Bangweulu</rdfs:label>
    </owl:NamedIndividual>
    


    <!-- http://purl.obolibrary.org/obo/GAZ_00049227 -->

    <owl:NamedIndividual rdf:about="http://purl.obolibrary.org/obo/GAZ_00049227">
        <obo:IAO_0000115>A lake.</obo:IAO_0000115>
        <oboInOwl:hasOBONamespace>GAZ</oboInOwl:hasOBONamespace>
        <oboInOwl:id>GAZ:00049227</oboInOwl:id>
        <rdfs:label>Lake Chali</rdfs:label>
    </owl:NamedIndividual>
    


    <!-- http://purl.obolibrary.org/obo/GAZ_00049228 -->

    <owl:NamedIndividual rdf:about="http://purl.obolibrary.org/obo/GAZ_00049228">
        <oboInOwl:hasOBONamespace>GAZ</oboInOwl:hasOBONamespace>
        <oboInOwl:id>GAZ:00049228</oboInOwl:id>
        <rdfs:label>Lake Chaya</rdfs:label>
    </owl:NamedIndividual>
    


    <!-- http://purl.obolibrary.org/obo/GAZ_00049229 -->

    <owl:NamedIndividual rdf:about="http://purl.obolibrary.org/obo/GAZ_00049229">
        <oboInOwl:hasOBONamespace>GAZ</oboInOwl:hasOBONamespace>
        <oboInOwl:id>GAZ:00049229</oboInOwl:id>
        <rdfs:label>Lake Wumba</rdfs:label>
    </owl:NamedIndividual>
    


    <!-- http://purl.obolibrary.org/obo/GAZ_00049230 -->

    <owl:NamedIndividual rdf:about="http://purl.obolibrary.org/obo/GAZ_00049230">
        <oboInOwl:hasOBONamespace>GAZ</oboInOwl:hasOBONamespace>
        <oboInOwl:id>GAZ:00049230</oboInOwl:id>
        <rdfs:label>Pook Lagoon</rdfs:label>
    </owl:NamedIndividual>
    


    <!-- http://purl.obolibrary.org/obo/GAZ_00049232 -->

    <owl:NamedIndividual rdf:about="http://purl.obolibrary.org/obo/GAZ_00049232">
        <obo:RO_0001025 rdf:resource="http://purl.obolibrary.org/obo/GAZ_00015182"/>
        <obo:RO_0001025 rdf:resource="http://purl.obolibrary.org/obo/GAZ_00049226"/>
        <obo:IAO_0000115>An island in Lake Bangweulu.</obo:IAO_0000115>
        <oboInOwl:hasOBONamespace>GAZ</oboInOwl:hasOBONamespace>
        <oboInOwl:id>GAZ:00049232</oboInOwl:id>
        <rdfs:label>Chilubi Island</rdfs:label>
    </owl:NamedIndividual>
    


    <!-- http://purl.obolibrary.org/obo/GAZ_00049233 -->

    <owl:NamedIndividual rdf:about="http://purl.obolibrary.org/obo/GAZ_00049233">
        <obo:RO_0001025 rdf:resource="http://purl.obolibrary.org/obo/GAZ_00049226"/>
        <oboInOwl:hasOBONamespace>GAZ</oboInOwl:hasOBONamespace>
        <oboInOwl:id>GAZ:00049233</oboInOwl:id>
        <rdfs:label>Mbabala Island</rdfs:label>
    </owl:NamedIndividual>
    


    <!-- http://purl.obolibrary.org/obo/GAZ_00049234 -->

    <owl:NamedIndividual rdf:about="http://purl.obolibrary.org/obo/GAZ_00049234">
        <oboInOwl:hasOBONamespace>GAZ</oboInOwl:hasOBONamespace>
        <oboInOwl:id>GAZ:00049234</oboInOwl:id>
        <rdfs:label>Lake Walilupe</rdfs:label>
    </owl:NamedIndividual>
    


    <!-- http://purl.obolibrary.org/obo/GAZ_00049235 -->

    <owl:NamedIndividual rdf:about="http://purl.obolibrary.org/obo/GAZ_00049235">
        <obo:RO_0001025 rdf:resource="http://purl.obolibrary.org/obo/GAZ_00049226"/>
        <oboInOwl:hasOBONamespace>GAZ</oboInOwl:hasOBONamespace>
        <oboInOwl:id>GAZ:00049235</oboInOwl:id>
        <rdfs:label>Chishi Island</rdfs:label>
    </owl:NamedIndividual>
    


    <!-- http://purl.obolibrary.org/obo/GAZ_00049236 -->

    <owl:NamedIndividual rdf:about="http://purl.obolibrary.org/obo/GAZ_00049236">
        <obo:RO_0001025 rdf:resource="http://purl.obolibrary.org/obo/GAZ_00049226"/>
        <oboInOwl:hasOBONamespace>GAZ</oboInOwl:hasOBONamespace>
        <oboInOwl:id>GAZ:00049236</oboInOwl:id>
        <rdfs:label>Lifunge Mwenzi Island</rdfs:label>
    </owl:NamedIndividual>
    


    <!-- http://purl.obolibrary.org/obo/GAZ_00049237 -->

    <owl:NamedIndividual rdf:about="http://purl.obolibrary.org/obo/GAZ_00049237">
        <oboInOwl:hasOBONamespace>GAZ</oboInOwl:hasOBONamespace>
        <oboInOwl:id>GAZ:00049237</oboInOwl:id>
        <rdfs:label>Lake Chifunabuli</rdfs:label>
    </owl:NamedIndividual>
    


    <!-- http://purl.obolibrary.org/obo/GAZ_00049238 -->

    <owl:NamedIndividual rdf:about="http://purl.obolibrary.org/obo/GAZ_00049238">
        <obo:RO_0001025 rdf:resource="http://purl.obolibrary.org/obo/GAZ_00049226"/>
        <oboInOwl:hasOBONamespace>GAZ</oboInOwl:hasOBONamespace>
        <oboInOwl:id>GAZ:00049238</oboInOwl:id>
        <rdfs:label>Chindo Island</rdfs:label>
    </owl:NamedIndividual>
    


    <!-- http://purl.obolibrary.org/obo/GAZ_00049239 -->

    <owl:NamedIndividual rdf:about="http://purl.obolibrary.org/obo/GAZ_00049239">
        <obo:RO_0001025 rdf:resource="http://purl.obolibrary.org/obo/GAZ_00049226"/>
        <oboInOwl:hasOBONamespace>GAZ</oboInOwl:hasOBONamespace>
        <oboInOwl:id>GAZ:00049239</oboInOwl:id>
        <rdfs:label>Ibula Island</rdfs:label>
    </owl:NamedIndividual>
    


    <!-- http://purl.obolibrary.org/obo/GAZ_00049240 -->

    <owl:NamedIndividual rdf:about="http://purl.obolibrary.org/obo/GAZ_00049240">
        <obo:RO_0001025 rdf:resource="http://purl.obolibrary.org/obo/GAZ_00049226"/>
        <oboInOwl:hasOBONamespace>GAZ</oboInOwl:hasOBONamespace>
        <oboInOwl:id>GAZ:00049240</oboInOwl:id>
        <rdfs:label>Chibwe Ngombe Island</rdfs:label>
    </owl:NamedIndividual>
    


    <!-- http://purl.obolibrary.org/obo/GAZ_00049241 -->

    <owl:NamedIndividual rdf:about="http://purl.obolibrary.org/obo/GAZ_00049241">
        <oboInOwl:hasOBONamespace>GAZ</oboInOwl:hasOBONamespace>
        <oboInOwl:id>GAZ:00049241</oboInOwl:id>
        <rdfs:label>Nsalushi Island</rdfs:label>
    </owl:NamedIndividual>
    


    <!-- http://purl.obolibrary.org/obo/GAZ_00049242 -->

    <owl:NamedIndividual rdf:about="http://purl.obolibrary.org/obo/GAZ_00049242">
        <oboInOwl:hasOBONamespace>GAZ</oboInOwl:hasOBONamespace>
        <oboInOwl:id>GAZ:00049242</oboInOwl:id>
        <rdfs:label>Nsumpa Island</rdfs:label>
    </owl:NamedIndividual>
    


    <!-- http://purl.obolibrary.org/obo/GAZ_00049243 -->

    <owl:NamedIndividual rdf:about="http://purl.obolibrary.org/obo/GAZ_00049243">
        <obo:IAO_0000115>An island.</obo:IAO_0000115>
        <oboInOwl:hasOBONamespace>GAZ</oboInOwl:hasOBONamespace>
        <oboInOwl:id>GAZ:00049243</oboInOwl:id>
        <rdfs:label>Nsumbu Island</rdfs:label>
    </owl:NamedIndividual>
    


    <!-- http://purl.obolibrary.org/obo/GAZ_00049244 -->

    <owl:NamedIndividual rdf:about="http://purl.obolibrary.org/obo/GAZ_00049244">
        <oboInOwl:hasOBONamespace>GAZ</oboInOwl:hasOBONamespace>
        <oboInOwl:id>GAZ:00049244</oboInOwl:id>
        <rdfs:label>Kawulu Island</rdfs:label>
    </owl:NamedIndividual>
    


    <!-- http://purl.obolibrary.org/obo/GAZ_00049245 -->

    <owl:NamedIndividual rdf:about="http://purl.obolibrary.org/obo/GAZ_00049245">
        <oboInOwl:hasOBONamespace>GAZ</oboInOwl:hasOBONamespace>
        <oboInOwl:id>GAZ:00049245</oboInOwl:id>
        <rdfs:label>Matonga Island</rdfs:label>
    </owl:NamedIndividual>
    


    <!-- http://purl.obolibrary.org/obo/GAZ_00049246 -->

    <owl:NamedIndividual rdf:about="http://purl.obolibrary.org/obo/GAZ_00049246">
        <oboInOwl:hasOBONamespace>GAZ</oboInOwl:hasOBONamespace>
        <oboInOwl:id>GAZ:00049246</oboInOwl:id>
        <rdfs:label>Munyanga Island</rdfs:label>
    </owl:NamedIndividual>
    


    <!-- http://purl.obolibrary.org/obo/GAZ_00049247 -->

    <owl:NamedIndividual rdf:about="http://purl.obolibrary.org/obo/GAZ_00049247">
        <obo:IAO_0000115>An island.</obo:IAO_0000115>
        <oboInOwl:hasOBONamespace>GAZ</oboInOwl:hasOBONamespace>
        <oboInOwl:id>GAZ:00049247</oboInOwl:id>
        <rdfs:label>Panyo Island</rdfs:label>
    </owl:NamedIndividual>
    


    <!-- http://purl.obolibrary.org/obo/GAZ_00049248 -->

    <owl:NamedIndividual rdf:about="http://purl.obolibrary.org/obo/GAZ_00049248">
        <oboInOwl:hasOBONamespace>GAZ</oboInOwl:hasOBONamespace>
        <oboInOwl:id>GAZ:00049248</oboInOwl:id>
        <rdfs:label>Mutwamina Island</rdfs:label>
    </owl:NamedIndividual>
    


    <!-- http://purl.obolibrary.org/obo/GAZ_00049249 -->

    <owl:NamedIndividual rdf:about="http://purl.obolibrary.org/obo/GAZ_00049249">
        <oboInOwl:hasOBONamespace>GAZ</oboInOwl:hasOBONamespace>
        <oboInOwl:id>GAZ:00049249</oboInOwl:id>
        <rdfs:label>Ncheta Island</rdfs:label>
    </owl:NamedIndividual>
    


    <!-- http://purl.obolibrary.org/obo/GAZ_00049250 -->

    <owl:NamedIndividual rdf:about="http://purl.obolibrary.org/obo/GAZ_00049250">
        <oboInOwl:hasOBONamespace>GAZ</oboInOwl:hasOBONamespace>
        <oboInOwl:id>GAZ:00049250</oboInOwl:id>
        <rdfs:label>Chisale Island</rdfs:label>
    </owl:NamedIndividual>
    


    <!-- http://purl.obolibrary.org/obo/GAZ_00052622 -->

    <owl:NamedIndividual rdf:about="http://purl.obolibrary.org/obo/GAZ_00052622">
        <rdf:type rdf:resource="http://purl.obolibrary.org/obo/ENVO_00000856"/>
        <obo:RO_0001025 rdf:resource="http://purl.obolibrary.org/obo/GAZ_00015169"/>
    </owl:NamedIndividual>
    


    <!-- http://purl.obolibrary.org/obo/GAZ_00052623 -->

    <owl:NamedIndividual rdf:about="http://purl.obolibrary.org/obo/GAZ_00052623">
        <rdf:type rdf:resource="http://purl.obolibrary.org/obo/ENVO_00000856"/>
        <obo:RO_0001025 rdf:resource="http://purl.obolibrary.org/obo/GAZ_00015175"/>
    </owl:NamedIndividual>
    


    <!-- http://purl.obolibrary.org/obo/GAZ_00052624 -->

    <owl:NamedIndividual rdf:about="http://purl.obolibrary.org/obo/GAZ_00052624">
        <obo:RO_0001025 rdf:resource="http://purl.obolibrary.org/obo/GAZ_00015174"/>
    </owl:NamedIndividual>
    


    <!-- http://purl.obolibrary.org/obo/GAZ_00052625 -->

    <owl:NamedIndividual rdf:about="http://purl.obolibrary.org/obo/GAZ_00052625">
        <obo:RO_0001025 rdf:resource="http://purl.obolibrary.org/obo/GAZ_00015187"/>
        <obo:RO_0001025 rdf:resource="http://purl.obolibrary.org/obo/GAZ_00015197"/>
    </owl:NamedIndividual>
    


    <!-- http://purl.obolibrary.org/obo/GAZ_00052626 -->

    <owl:NamedIndividual rdf:about="http://purl.obolibrary.org/obo/GAZ_00052626">
        <obo:RO_0001025 rdf:resource="http://purl.obolibrary.org/obo/GAZ_00009423"/>
        <obo:IAO_0000115>A national park that lies on the western shore of Lake Tanganyika near its southern extremity, in Zambia&apos;s Northern Province. It covers about 2000 km2 and has some 80 km of lake shore including four bays (Kasaba, Kala, Nkamba and Sumbu), and Nundo Head Peninsula.</obo:IAO_0000115>
        <oboInOwl:hasOBONamespace>GAZ</oboInOwl:hasOBONamespace>
        <oboInOwl:id>GAZ:00052626</oboInOwl:id>
        <rdfs:label>Nsumbu National Park</rdfs:label>
    </owl:NamedIndividual>
    


    <!-- http://purl.obolibrary.org/obo/GAZ_00052627 -->

    <owl:NamedIndividual rdf:about="http://purl.obolibrary.org/obo/GAZ_00052627">
        <obo:RO_0001025 rdf:resource="http://purl.obolibrary.org/obo/GAZ_00010009"/>
        <oboInOwl:hasOBONamespace>GAZ</oboInOwl:hasOBONamespace>
        <oboInOwl:id>GAZ:00052627</oboInOwl:id>
        <rdfs:label>University (of Zambia) Teaching Hospital</rdfs:label>
    </owl:NamedIndividual>
    


    <!-- http://purl.obolibrary.org/obo/GAZ_00052628 -->

    <owl:NamedIndividual rdf:about="http://purl.obolibrary.org/obo/GAZ_00052628">
        <rdf:type rdf:resource="http://purl.obolibrary.org/obo/ENVO_00000856"/>
        <obo:RO_0001025 rdf:resource="http://purl.obolibrary.org/obo/GAZ_00015158"/>
    </owl:NamedIndividual>
    


    <!-- http://purl.obolibrary.org/obo/GAZ_00052629 -->

    <owl:NamedIndividual rdf:about="http://purl.obolibrary.org/obo/GAZ_00052629">
        <obo:IAO_0000115>A river that is a major tributary of the Zambezi River. The Luwangwa rises in the Lilonda and Mafinga Hills in north-east Zambia at an elevation of around 1500 m, near the border with Tanzania and Malawi, and flows in a southwesterly direction through a broad valley. About 150 km from its source it has dropped to an elevation of about 690 m and becomes a meandering river with a flood-plain several km wide. Over the next 300 km the meanders increase, with many ox-bow lakes and abandoned meanders. Near Mfuwe, the river&apos;s elevation has dropped to about 520 m, the flood plain is about 10 km wide and the valley reaches about 100 km wide, with a north-west escarpment (Muchinga Escarpment) about 700 m high, and a south-western escarpment about 450 m high. In the dry season some sections, especially in the upper reaches, dry out completely, leaving isolated pools. At about 500 km the valley narrows to about 50 km and becomes divided by a ridge into two parallel valleys, with a tributary, the Lukusashi River in a 25 km-wide valley to the north-west, and the Luangwa in a 15 km wide valley to the southeast. The river meanders less, and the flood plain narrows. At 600 km the river abruptly enters a narrow valley between hills rising some 200 m from the broader valley floor, becoming almost a gorge. About 700 km from source the Luangwa merges with its tributary the Lukusashi after the latter has merged with the Lunsemfwa River coming from the oppostie driection, and turns due south through a steep narrow valley: this is its exit from the Luangwa Rift Valley (see following section). After only 20 km it emerges from the hills into the broad valley of the Zambezi and meanders over sandy flats about 1.5 km wide in a flood plain of 3-5 km wide. It merges with the deeper Zambezi at Luangwa town.</obo:IAO_0000115>
        <oboInOwl:hasOBONamespace>GAZ</oboInOwl:hasOBONamespace>
        <oboInOwl:id>GAZ:00052629</oboInOwl:id>
        <rdfs:label>Luangwa River</rdfs:label>
    </owl:NamedIndividual>
    


    <!-- http://purl.obolibrary.org/obo/GAZ_00052631 -->

    <owl:NamedIndividual rdf:about="http://purl.obolibrary.org/obo/GAZ_00052631">
        <obo:RO_0001025 rdf:resource="http://purl.obolibrary.org/obo/GAZ_00009423"/>
    </owl:NamedIndividual>
    


    <!-- http://purl.obolibrary.org/obo/GAZ_00052632 -->

    <owl:NamedIndividual rdf:about="http://purl.obolibrary.org/obo/GAZ_00052632">
        <obo:IAO_0000115>The gorges below the Victoria Falls.</obo:IAO_0000115>
        <oboInOwl:hasOBONamespace>GAZ</oboInOwl:hasOBONamespace>
        <oboInOwl:id>GAZ:00052632</oboInOwl:id>
        <rdfs:label>Victoria Falls Gorges</rdfs:label>
    </owl:NamedIndividual>
    


    <!-- http://purl.obolibrary.org/obo/GAZ_00052634 -->

    <owl:NamedIndividual rdf:about="http://purl.obolibrary.org/obo/GAZ_00052634">
        <obo:RO_0001025 rdf:resource="http://purl.obolibrary.org/obo/GAZ_00052632"/>
        <oboInOwl:hasOBONamespace>GAZ</oboInOwl:hasOBONamespace>
        <oboInOwl:id>GAZ:00052634</oboInOwl:id>
        <rdfs:label>Fifth Gorge</rdfs:label>
    </owl:NamedIndividual>
    


    <!-- http://purl.obolibrary.org/obo/GAZ_00052635 -->

    <owl:NamedIndividual rdf:about="http://purl.obolibrary.org/obo/GAZ_00052635">
        <obo:RO_0001025 rdf:resource="http://purl.obolibrary.org/obo/GAZ_00052632"/>
        <oboInOwl:hasOBONamespace>GAZ</oboInOwl:hasOBONamespace>
        <oboInOwl:id>GAZ:00052635</oboInOwl:id>
        <rdfs:label>Third Gorge</rdfs:label>
    </owl:NamedIndividual>
    


    <!-- http://purl.obolibrary.org/obo/GAZ_00052636 -->

    <owl:NamedIndividual rdf:about="http://purl.obolibrary.org/obo/GAZ_00052636">
        <obo:RO_0001025 rdf:resource="http://purl.obolibrary.org/obo/GAZ_00052632"/>
        <oboInOwl:hasOBONamespace>GAZ</oboInOwl:hasOBONamespace>
        <oboInOwl:id>GAZ:00052636</oboInOwl:id>
        <rdfs:label>Songwe Gorge</rdfs:label>
    </owl:NamedIndividual>
    


    <!-- http://purl.obolibrary.org/obo/GAZ_00052637 -->

    <owl:NamedIndividual rdf:about="http://purl.obolibrary.org/obo/GAZ_00052637">
        <obo:RO_0001025 rdf:resource="http://purl.obolibrary.org/obo/GAZ_00052632"/>
        <oboInOwl:hasOBONamespace>GAZ</oboInOwl:hasOBONamespace>
        <oboInOwl:id>GAZ:00052637</oboInOwl:id>
        <rdfs:label>Batoka Gorge</rdfs:label>
    </owl:NamedIndividual>
    


    <!-- http://purl.obolibrary.org/obo/GAZ_00052638 -->

    <owl:NamedIndividual rdf:about="http://purl.obolibrary.org/obo/GAZ_00052638">
        <obo:RO_0001025 rdf:resource="http://purl.obolibrary.org/obo/GAZ_00052632"/>
        <oboInOwl:hasOBONamespace>GAZ</oboInOwl:hasOBONamespace>
        <oboInOwl:id>GAZ:00052638</oboInOwl:id>
        <rdfs:label>First Gorge</rdfs:label>
    </owl:NamedIndividual>
    


    <!-- http://purl.obolibrary.org/obo/GAZ_00052639 -->

    <owl:NamedIndividual rdf:about="http://purl.obolibrary.org/obo/GAZ_00052639">
        <obo:RO_0001025 rdf:resource="http://purl.obolibrary.org/obo/GAZ_00052632"/>
        <oboInOwl:hasOBONamespace>GAZ</oboInOwl:hasOBONamespace>
        <oboInOwl:id>GAZ:00052639</oboInOwl:id>
        <rdfs:label>Fourth Gorge</rdfs:label>
    </owl:NamedIndividual>
    


    <!-- http://purl.obolibrary.org/obo/GAZ_00052640 -->

    <owl:NamedIndividual rdf:about="http://purl.obolibrary.org/obo/GAZ_00052640">
        <obo:RO_0001025 rdf:resource="http://purl.obolibrary.org/obo/GAZ_00052632"/>
        <oboInOwl:hasOBONamespace>GAZ</oboInOwl:hasOBONamespace>
        <oboInOwl:id>GAZ:00052640</oboInOwl:id>
        <rdfs:label>Second Gorge</rdfs:label>
    </owl:NamedIndividual>
    


    <!-- http://purl.obolibrary.org/obo/GAZ_00052641 -->

    <owl:NamedIndividual rdf:about="http://purl.obolibrary.org/obo/GAZ_00052641">
        <rdf:type rdf:resource="http://purl.obolibrary.org/obo/ENVO_00000856"/>
        <obo:RO_0001025 rdf:resource="http://purl.obolibrary.org/obo/GAZ_00015202"/>
    </owl:NamedIndividual>
    


    <!-- http://purl.obolibrary.org/obo/GAZ_00052642 -->

    <owl:NamedIndividual rdf:about="http://purl.obolibrary.org/obo/GAZ_00052642">
        <obo:IAO_0000115>A flat plateau at an elevation of about 1000 m tilting very slightly to the south. The Zambezi and its headwaters rise on the higher ground to the north, which enjoys good rainfall (1400 mm annually) in a rainy season from October to May. A flood moves down the river reaching a flat region, formed from Kalahari sands, about 500 km across. To the south around the Ngonye Falls harder rock is found at the surface and has resisted the river&apos;s tendency to cut a channel down into it, and so acts a bit like a dam. Behind it the floodplain has formed.</obo:IAO_0000115>
        <oboInOwl:hasOBONamespace>GAZ</oboInOwl:hasOBONamespace>
        <oboInOwl:id>GAZ:00052642</oboInOwl:id>
        <rdfs:label>Barotse Floodplain</rdfs:label>
    </owl:NamedIndividual>
    


    <!-- http://purl.obolibrary.org/obo/GAZ_00052643 -->

    <owl:NamedIndividual rdf:about="http://purl.obolibrary.org/obo/GAZ_00052643">
        <obo:RO_0001025 rdf:resource="http://purl.obolibrary.org/obo/GAZ_00015190"/>
    </owl:NamedIndividual>
    


    <!-- http://purl.obolibrary.org/obo/GAZ_00052644 -->

    <owl:NamedIndividual rdf:about="http://purl.obolibrary.org/obo/GAZ_00052644">
        <obo:RO_0001025 rdf:resource="http://purl.obolibrary.org/obo/GAZ_00015141"/>
    </owl:NamedIndividual>
    


    <!-- http://purl.obolibrary.org/obo/GAZ_00052645 -->

    <owl:NamedIndividual rdf:about="http://purl.obolibrary.org/obo/GAZ_00052645">
        <obo:RO_0001025 rdf:resource="http://purl.obolibrary.org/obo/GAZ_00015195"/>
    </owl:NamedIndividual>
    


    <!-- http://purl.obolibrary.org/obo/GAZ_00052646 -->

    <owl:NamedIndividual rdf:about="http://purl.obolibrary.org/obo/GAZ_00052646">
        <obo:IAO_0000115>A national park that lies south west of Lusaka in Zambia, on the south side of the Kafue River. The national park straddles two of Zambia&apos;s ecoregions: Zambezian and Mopane woodlands in the south, and Zambezian flooded grasslands over most of the park. Habitats in the latter ecoregion include Chunga Lagoon and the Kafue Flats (floodplain), and drier grassland between floodplain and woodland dominated by termite mounds.</obo:IAO_0000115>
        <oboInOwl:hasOBONamespace>GAZ</oboInOwl:hasOBONamespace>
        <oboInOwl:id>GAZ:00052646</oboInOwl:id>
        <rdfs:label>Lochinvar National Park</rdfs:label>
    </owl:NamedIndividual>
    


    <!-- http://purl.obolibrary.org/obo/GAZ_00052647 -->

    <owl:NamedIndividual rdf:about="http://purl.obolibrary.org/obo/GAZ_00052647">
        <obo:RO_0001025 rdf:resource="http://purl.obolibrary.org/obo/GAZ_00015187"/>
    </owl:NamedIndividual>
    


    <!-- http://purl.obolibrary.org/obo/GAZ_00052649 -->

    <owl:NamedIndividual rdf:about="http://purl.obolibrary.org/obo/GAZ_00052649">
        <obo:RO_0001025 rdf:resource="http://purl.obolibrary.org/obo/GAZ_00015193"/>
        <obo:IAO_0000115>A dam on the Kafue River in west-central Zambia at the Itezhi-Tezhi Gap, in a range of hills through which the river had eroded a narrow valley, leading to the broad expanse of the wetlands known as the Kafue Flats. Constructed 1974-1977.</obo:IAO_0000115>
        <oboInOwl:hasOBONamespace>GAZ</oboInOwl:hasOBONamespace>
        <oboInOwl:id>GAZ:00052649</oboInOwl:id>
        <rdfs:label>Itezhi-Tezhi Dam</rdfs:label>
    </owl:NamedIndividual>
    


    <!-- http://purl.obolibrary.org/obo/GAZ_00052651 -->

    <owl:NamedIndividual rdf:about="http://purl.obolibrary.org/obo/GAZ_00052651">
        <rdf:type rdf:resource="http://purl.obolibrary.org/obo/ENVO_00000856"/>
        <obo:RO_0001025 rdf:resource="http://purl.obolibrary.org/obo/GAZ_00015197"/>
    </owl:NamedIndividual>
    


    <!-- http://purl.obolibrary.org/obo/GAZ_00052652 -->

    <owl:NamedIndividual rdf:about="http://purl.obolibrary.org/obo/GAZ_00052652">
        <obo:IAO_0000115>A large, natural gorge through which flowed the Zambezi River on the border of Zambia and Zimbabwe, Africa.</obo:IAO_0000115>
        <oboInOwl:hasOBONamespace>GAZ</oboInOwl:hasOBONamespace>
        <oboInOwl:id>GAZ:00052652</oboInOwl:id>
        <rdfs:label>Kariba Gorge</rdfs:label>
    </owl:NamedIndividual>
    


    <!-- http://purl.obolibrary.org/obo/GAZ_00052653 -->

    <owl:NamedIndividual rdf:about="http://purl.obolibrary.org/obo/GAZ_00052653">
        <obo:RO_0001025 rdf:resource="http://purl.obolibrary.org/obo/GAZ_00052652"/>
        <obo:IAO_0000115>A hydroelectric dam in the Kariba Gorge of the Zambezi river basin between Zambia and Zimbabwe.</obo:IAO_0000115>
        <oboInOwl:hasOBONamespace>GAZ</oboInOwl:hasOBONamespace>
        <oboInOwl:id>GAZ:00052653</oboInOwl:id>
        <rdfs:label>Kariba Dam</rdfs:label>
    </owl:NamedIndividual>
    


    <!-- http://purl.obolibrary.org/obo/GAZ_00052654 -->

    <owl:NamedIndividual rdf:about="http://purl.obolibrary.org/obo/GAZ_00052654">
        <rdf:type rdf:resource="http://purl.obolibrary.org/obo/ENVO_00000856"/>
        <obo:RO_0001025 rdf:resource="http://purl.obolibrary.org/obo/GAZ_00015178"/>
    </owl:NamedIndividual>
    


    <!-- http://purl.obolibrary.org/obo/GAZ_00052655 -->

    <owl:NamedIndividual rdf:about="http://purl.obolibrary.org/obo/GAZ_00052655">
        <rdf:type rdf:resource="http://purl.obolibrary.org/obo/ENVO_00000856"/>
        <obo:RO_0001025 rdf:resource="http://purl.obolibrary.org/obo/GAZ_00009430"/>
    </owl:NamedIndividual>
    


    <!-- http://purl.obolibrary.org/obo/GAZ_00052656 -->

    <owl:NamedIndividual rdf:about="http://purl.obolibrary.org/obo/GAZ_00052656">
        <obo:RO_0001025 rdf:resource="http://purl.obolibrary.org/obo/GAZ_00015144"/>
    </owl:NamedIndividual>
    


    <!-- http://purl.obolibrary.org/obo/GAZ_00052657 -->

    <owl:NamedIndividual rdf:about="http://purl.obolibrary.org/obo/GAZ_00052657">
        <obo:RO_0001025 rdf:resource="http://purl.obolibrary.org/obo/GAZ_00009423"/>
        <obo:IAO_0000115>A land-tied island in Northern Province, Zambia.</obo:IAO_0000115>
        <oboInOwl:hasOBONamespace>GAZ</oboInOwl:hasOBONamespace>
        <oboInOwl:id>GAZ:00052657</oboInOwl:id>
        <rdfs:label>Inangu Peninsula</rdfs:label>
    </owl:NamedIndividual>
    


    <!-- http://purl.obolibrary.org/obo/GAZ_00052658 -->

    <owl:NamedIndividual rdf:about="http://purl.obolibrary.org/obo/GAZ_00052658">
        <rdf:type rdf:resource="http://purl.obolibrary.org/obo/ENVO_00000062"/>
        <obo:RO_0001025 rdf:resource="http://purl.obolibrary.org/obo/GAZ_00015174"/>
        <obo:IAO_0000115>A place.</obo:IAO_0000115>
        <oboInOwl:hasOBONamespace>GAZ</oboInOwl:hasOBONamespace>
        <oboInOwl:id>GAZ:00052658</oboInOwl:id>
        <rdfs:label>Kapembwa</rdfs:label>
    </owl:NamedIndividual>
    


    <!-- http://purl.obolibrary.org/obo/GAZ_00052659 -->

    <owl:NamedIndividual rdf:about="http://purl.obolibrary.org/obo/GAZ_00052659">
        <rdf:type rdf:resource="http://purl.obolibrary.org/obo/ENVO_00000062"/>
        <obo:RO_0001025 rdf:resource="http://purl.obolibrary.org/obo/GAZ_00015174"/>
        <obo:IAO_0000115>A place.</obo:IAO_0000115>
        <oboInOwl:hasOBONamespace>GAZ</oboInOwl:hasOBONamespace>
        <oboInOwl:id>GAZ:00052659</oboInOwl:id>
        <rdfs:label>Kasakalawe</rdfs:label>
    </owl:NamedIndividual>
    


    <!-- http://purl.obolibrary.org/obo/GAZ_00052661 -->

    <owl:NamedIndividual rdf:about="http://purl.obolibrary.org/obo/GAZ_00052661">
        <rdf:type rdf:resource="http://purl.obolibrary.org/obo/ENVO_00000856"/>
        <obo:RO_0001025 rdf:resource="http://purl.obolibrary.org/obo/GAZ_00015177"/>
    </owl:NamedIndividual>
    


    <!-- http://purl.obolibrary.org/obo/GAZ_00058777 -->

    <owl:NamedIndividual rdf:about="http://purl.obolibrary.org/obo/GAZ_00058777">
        <obo:RO_0001025 rdf:resource="http://purl.obolibrary.org/obo/GAZ_00009425"/>
        <obo:IAO_0000115>A lake situated south-west of Luanshya, Zambia.</obo:IAO_0000115>
        <oboInOwl:hasOBONamespace>GAZ</oboInOwl:hasOBONamespace>
        <oboInOwl:id>GAZ:00058777</oboInOwl:id>
        <rdfs:label>Lake Kashiba</rdfs:label>
    </owl:NamedIndividual>
    


    <!-- http://purl.obolibrary.org/obo/GAZ_00058778 -->

    <owl:NamedIndividual rdf:about="http://purl.obolibrary.org/obo/GAZ_00058778">
        <obo:RO_0001025 rdf:resource="http://purl.obolibrary.org/obo/GAZ_00009423"/>
        <obo:IAO_0000115>A lake very close to the watershed between the Luangwa and Chambeshi River basins in the Northern Province of Zambia, and just on the Chambeshi side.</obo:IAO_0000115>
        <oboInOwl:hasOBONamespace>GAZ</oboInOwl:hasOBONamespace>
        <oboInOwl:id>GAZ:00058778</oboInOwl:id>
        <rdfs:label>Lake Ishiba Ng&apos;andu</rdfs:label>
    </owl:NamedIndividual>
    


    <!-- http://purl.obolibrary.org/obo/GAZ_00058780 -->

    <owl:NamedIndividual rdf:about="http://purl.obolibrary.org/obo/GAZ_00058780">
        <obo:RO_0001025 rdf:resource="http://purl.obolibrary.org/obo/GAZ_00009427"/>
        <obo:RO_0001025 rdf:resource="http://purl.obolibrary.org/obo/GAZ_00058782"/>
        <obo:IAO_0000115>A lake lagoon in Zambia. It is the largest of several lagoons in the Luapula River swamps south of Lake Mweru, in the Luapula Province of Zambia.</obo:IAO_0000115>
        <oboInOwl:hasOBONamespace>GAZ</oboInOwl:hasOBONamespace>
        <oboInOwl:id>GAZ:00058780</oboInOwl:id>
        <rdfs:label>Mofwe Lagoon</rdfs:label>
    </owl:NamedIndividual>
    


    <!-- http://purl.obolibrary.org/obo/GAZ_00058781 -->

    <owl:NamedIndividual rdf:about="http://purl.obolibrary.org/obo/GAZ_00058781">
        <obo:RO_0001025 rdf:resource="http://purl.obolibrary.org/obo/GAZ_00009427"/>
        <obo:IAO_0000115>A river that drains the northern Zambian plateau north of Kawambwa and flows west into the Luapula valley. It enters the Luapula swamps near the Mofwe Lagoon.</obo:IAO_0000115>
        <oboInOwl:hasOBONamespace>GAZ</oboInOwl:hasOBONamespace>
        <oboInOwl:id>GAZ:00058781</oboInOwl:id>
        <rdfs:label>Mbereshi River</rdfs:label>
    </owl:NamedIndividual>
    


    <!-- http://purl.obolibrary.org/obo/GAZ_00058782 -->

    <owl:NamedIndividual rdf:about="http://purl.obolibrary.org/obo/GAZ_00058782">
        <obo:IAO_0000115>Swamps that stretch along the last 100 km of the Luapula River before it reaches the Lake Mweru, and for much of that they are 30 km wide, covering and area of about 2500 km2. There are four inhabited islands in the DR Congo part of the delta, including the largest in the system which is connected to dry land in the dry season. Zambia has three inhabited islands in the delta including Chisenga Island. The are also many lagoons, the largest of which is Mofwe Lagoon on the Zambian side.</obo:IAO_0000115>
        <oboInOwl:hasOBONamespace>GAZ</oboInOwl:hasOBONamespace>
        <oboInOwl:id>GAZ:00058782</oboInOwl:id>
        <rdfs:label>Luapula Swamps</rdfs:label>
    </owl:NamedIndividual>
    


    <!-- http://purl.obolibrary.org/obo/GAZ_00058783 -->

    <owl:NamedIndividual rdf:about="http://purl.obolibrary.org/obo/GAZ_00058783">
        <obo:RO_0001025 rdf:resource="http://purl.obolibrary.org/obo/GAZ_00058782"/>
        <obo:IAO_0000115>A Zambian island in the Luapula Swamps.</obo:IAO_0000115>
        <oboInOwl:hasOBONamespace>GAZ</oboInOwl:hasOBONamespace>
        <oboInOwl:id>GAZ:00058783</oboInOwl:id>
        <rdfs:label>Chisenga Island</rdfs:label>
    </owl:NamedIndividual>
    


    <!-- http://purl.obolibrary.org/obo/GAZ_00058784 -->

    <owl:NamedIndividual rdf:about="http://purl.obolibrary.org/obo/GAZ_00058784">
        <obo:RO_0001025 rdf:resource="http://purl.obolibrary.org/obo/GAZ_00058785"/>
        <obo:IAO_0000115>A reservoir SE of Kabwe, Zambia due to the construction by the Broken Hill Development Company of the Mulungushi Dam on the Mulungushi River. Completed 1925.</obo:IAO_0000115>
        <oboInOwl:hasOBONamespace>GAZ</oboInOwl:hasOBONamespace>
        <oboInOwl:id>GAZ:00058784</oboInOwl:id>
        <rdfs:label>Mulungushi Lake</rdfs:label>
    </owl:NamedIndividual>
    


    <!-- http://purl.obolibrary.org/obo/GAZ_00058785 -->

    <owl:NamedIndividual rdf:about="http://purl.obolibrary.org/obo/GAZ_00058785">
        <obo:RO_0001025 rdf:resource="http://purl.obolibrary.org/obo/GAZ_00009429"/>
        <obo:IAO_0000115>A river in central Zambia is a tributary of the Lunsemfwa River and the Luangwa River, and a part of the Zambezi River basin. It rises on the plateau north-west of Kabwe and flows south-east into the Luangwa Rift Valley where it joins the Lunsemfwa.</obo:IAO_0000115>
        <oboInOwl:hasOBONamespace>GAZ</oboInOwl:hasOBONamespace>
        <oboInOwl:id>GAZ:00058785</oboInOwl:id>
        <rdfs:label>Mulungushi River</rdfs:label>
    </owl:NamedIndividual>
    


    <!-- http://purl.obolibrary.org/obo/GAZ_00076592 -->

    <owl:NamedIndividual rdf:about="http://purl.obolibrary.org/obo/GAZ_00076592">
        <obo:IAO_0000115>A national park in Malawi.</obo:IAO_0000115>
        <oboInOwl:hasOBONamespace>GAZ</oboInOwl:hasOBONamespace>
        <oboInOwl:id>GAZ:00076592</oboInOwl:id>
        <rdfs:label>Nyika National Park [Malawi]</rdfs:label>
    </owl:NamedIndividual>
    


    <!-- http://purl.obolibrary.org/obo/GAZ_00076593 -->

    <owl:NamedIndividual rdf:about="http://purl.obolibrary.org/obo/GAZ_00076593">
        <obo:RO_0001025 rdf:resource="http://purl.obolibrary.org/obo/GAZ_00009423"/>
        <obo:IAO_0000115>A national park that lies in the northeast of Zambia, on the western edge of the Nyika Plateau, which is one of the highest parts of the country and most of which lies in neighbouring Malawi.</obo:IAO_0000115>
        <oboInOwl:hasOBONamespace>GAZ</oboInOwl:hasOBONamespace>
        <oboInOwl:id>GAZ:00076593</oboInOwl:id>
        <rdfs:label>Nyika National Park [Zambia]</rdfs:label>
    </owl:NamedIndividual>
    


    <!-- http://purl.obolibrary.org/obo/GAZ_00076736 -->

    <owl:NamedIndividual rdf:about="http://purl.obolibrary.org/obo/GAZ_00076736">
        <obo:RO_0001025 rdf:resource="http://purl.obolibrary.org/obo/GAZ_00009429"/>
        <obo:IAO_0000115>A small wildlife haven in the northern part of the Kafue Flats in Zambia&apos;s Central Province.</obo:IAO_0000115>
        <oboInOwl:hasOBONamespace>GAZ</oboInOwl:hasOBONamespace>
        <oboInOwl:id>GAZ:00076736</oboInOwl:id>
        <rdfs:label>Blue Lagoon National Park</rdfs:label>
    </owl:NamedIndividual>
    


    <!-- http://purl.obolibrary.org/obo/GAZ_00076737 -->

    <owl:NamedIndividual rdf:about="http://purl.obolibrary.org/obo/GAZ_00076737">
        <obo:RO_0001025 rdf:resource="http://purl.obolibrary.org/obo/GAZ_00015182"/>
        <obo:IAO_0000115>A national park located E of the Bangweulu Swamps.</obo:IAO_0000115>
        <oboInOwl:hasOBONamespace>GAZ</oboInOwl:hasOBONamespace>
        <oboInOwl:id>GAZ:00076737</oboInOwl:id>
        <rdfs:label>Isangano National Park</rdfs:label>
    </owl:NamedIndividual>
    


    <!-- http://purl.obolibrary.org/obo/GAZ_00076738 -->

    <owl:NamedIndividual rdf:about="http://purl.obolibrary.org/obo/GAZ_00076738">
        <obo:RO_0001025 rdf:resource="http://purl.obolibrary.org/obo/GAZ_00009429"/>
        <obo:IAO_0000115>A national park in Central Province, Zambia.</obo:IAO_0000115>
        <oboInOwl:hasOBONamespace>GAZ</oboInOwl:hasOBONamespace>
        <oboInOwl:id>GAZ:00076738</oboInOwl:id>
        <rdfs:label>Kasanka National Park</rdfs:label>
    </owl:NamedIndividual>
    


    <!-- http://purl.obolibrary.org/obo/GAZ_00076739 -->

    <owl:NamedIndividual rdf:about="http://purl.obolibrary.org/obo/GAZ_00076739">
        <obo:RO_0001025 rdf:resource="http://purl.obolibrary.org/obo/GAZ_00009423"/>
        <obo:IAO_0000115>A national park in Zambia, south-east of the Bangweulu Swamps.</obo:IAO_0000115>
        <oboInOwl:hasOBONamespace>GAZ</oboInOwl:hasOBONamespace>
        <oboInOwl:id>GAZ:00076739</oboInOwl:id>
        <rdfs:label>Lavushi Manda National Park</rdfs:label>
    </owl:NamedIndividual>
    


    <!-- http://purl.obolibrary.org/obo/GAZ_00076740 -->

    <owl:NamedIndividual rdf:about="http://purl.obolibrary.org/obo/GAZ_00076740">
        <obo:RO_0001025 rdf:resource="http://purl.obolibrary.org/obo/GAZ_00009430"/>
        <obo:RO_0001025 rdf:resource="http://purl.obolibrary.org/obo/GAZ_00052642"/>
        <obo:IAO_0000115>A national park that lies in Western Province, Zambia, west of the Barotse Floodplain of the Zambezi River near the border with Angola.</obo:IAO_0000115>
        <oboInOwl:hasOBONamespace>GAZ</oboInOwl:hasOBONamespace>
        <oboInOwl:id>GAZ:00076740</oboInOwl:id>
        <rdfs:label>Liuwa Plain National Park</rdfs:label>
    </owl:NamedIndividual>
    


    <!-- http://purl.obolibrary.org/obo/GAZ_00076741 -->

    <owl:NamedIndividual rdf:about="http://purl.obolibrary.org/obo/GAZ_00076741">
        <obo:RO_0001025 rdf:resource="http://purl.obolibrary.org/obo/GAZ_00009420"/>
        <obo:IAO_0000115>A national park that lies on the north bank of the Zambezi River in south eastern Zambia. It gently slopes from the Zambezi Escarpment down to the river, straddling two main woodland savannah ecoregions distinguished by the dominant types of tree, Miombo and Mopane: Southern Miombo woodlands on higher ground in the north, and Zambezian and Mopane woodlands on lower slopes in the south. At the edge of the river is floodplain habitat.</obo:IAO_0000115>
        <oboInOwl:hasOBONamespace>GAZ</oboInOwl:hasOBONamespace>
        <oboInOwl:id>GAZ:00076741</oboInOwl:id>
        <rdfs:label>Lower Zambezi National Park</rdfs:label>
    </owl:NamedIndividual>
    


    <!-- http://purl.obolibrary.org/obo/GAZ_00076742 -->

    <owl:NamedIndividual rdf:about="http://purl.obolibrary.org/obo/GAZ_00076742">
        <obo:RO_0001025 rdf:resource="http://purl.obolibrary.org/obo/GAZ_00009421"/>
        <obo:IAO_0000115>A national park located in the Eastern Province of Zambia. The park is situated north-east of the famous South Luangwa National Park, and south of the inaccessible North Luangwa National Park. Like its neighbours, it is located in the Luangwa River rift valley.</obo:IAO_0000115>
        <oboInOwl:hasOBONamespace>GAZ</oboInOwl:hasOBONamespace>
        <oboInOwl:id>GAZ:00076742</oboInOwl:id>
        <rdfs:label>Luambe National Park</rdfs:label>
    </owl:NamedIndividual>
    


    <!-- http://purl.obolibrary.org/obo/GAZ_00076743 -->

    <owl:NamedIndividual rdf:about="http://purl.obolibrary.org/obo/GAZ_00076743">
        <obo:RO_0001025 rdf:resource="http://purl.obolibrary.org/obo/GAZ_00009421"/>
        <obo:IAO_0000115>A national park located in eastern Luangwa Valley in Zambia, on the other side of the Luangwa River from the more famous South Luangwa National Park. It lies between the smaller Luambe National Park (on the eastern bank of the river) and the Chipata-Lundazi road.</obo:IAO_0000115>
        <oboInOwl:hasOBONamespace>GAZ</oboInOwl:hasOBONamespace>
        <oboInOwl:id>GAZ:00076743</oboInOwl:id>
        <rdfs:label>Lukusuzi National Park</rdfs:label>
    </owl:NamedIndividual>
    


    <!-- http://purl.obolibrary.org/obo/GAZ_00076744 -->

    <owl:NamedIndividual rdf:about="http://purl.obolibrary.org/obo/GAZ_00076744">
        <obo:RO_0001025 rdf:resource="http://purl.obolibrary.org/obo/GAZ_00009427"/>
        <obo:IAO_0000115>A national park east of Lake Mweru in Zambia.</obo:IAO_0000115>
        <oboInOwl:hasOBONamespace>GAZ</oboInOwl:hasOBONamespace>
        <oboInOwl:id>GAZ:00076744</oboInOwl:id>
        <rdfs:label>Lusenga Plain National Park</rdfs:label>
    </owl:NamedIndividual>
    


    <!-- http://purl.obolibrary.org/obo/GAZ_00076745 -->

    <owl:NamedIndividual rdf:about="http://purl.obolibrary.org/obo/GAZ_00076745">
        <obo:RO_0001025 rdf:resource="http://purl.obolibrary.org/obo/GAZ_00009422"/>
        <obo:IAO_0000115>A national park in Zambia at the Victoria Falls. The river forms the border between Zambia and Zimbabwe, so the falls is shared by the two countries, and the park is &apos;twin&apos; to the Victoria Falls National Park on the Zimbabwean side. Mosi-oa-Tunya National Park covers 66 km2 from the Songwe Gorge below the falls in a north-west arc along about 20 km of the Zambian river bank. It forms the south-western boundary of the city of Livingstone and has two main sections, each with separate entrances: a wildlife park at its north-western end, and the land adjacent to the Victoria Falls, which in the rainy season is the world&apos;s largest curtain of falling water. It extends downstream from the falls and to the south-east along the Batoka Gorges.</obo:IAO_0000115>
        <oboInOwl:hasOBONamespace>GAZ</oboInOwl:hasOBONamespace>
        <oboInOwl:id>GAZ:00076745</oboInOwl:id>
        <rdfs:label>Mosi-oa-Tunya National Park</rdfs:label>
    </owl:NamedIndividual>
    


    <!-- http://purl.obolibrary.org/obo/GAZ_00076746 -->

    <owl:NamedIndividual rdf:about="http://purl.obolibrary.org/obo/GAZ_00076746">
        <obo:RO_0001025 rdf:resource="http://purl.obolibrary.org/obo/GAZ_00009423"/>
        <obo:RO_0001025 rdf:resource="http://purl.obolibrary.org/obo/GAZ_00015159"/>
        <obo:IAO_0000115>A national park in Zambia.</obo:IAO_0000115>
        <oboInOwl:hasOBONamespace>GAZ</oboInOwl:hasOBONamespace>
        <oboInOwl:id>GAZ:00076746</oboInOwl:id>
        <rdfs:label>Mweru Wantipa National Park</rdfs:label>
    </owl:NamedIndividual>
    


    <!-- http://purl.obolibrary.org/obo/GAZ_00076747 -->

    <owl:NamedIndividual rdf:about="http://purl.obolibrary.org/obo/GAZ_00076747">
        <obo:RO_0001025 rdf:resource="http://purl.obolibrary.org/obo/GAZ_00009423"/>
        <obo:IAO_0000115>A national park in Zambia, the northernmost of the three in the valley of the Luangwa River. Founded as a game reserve in 1938, it became a national park in 1972. Like the South Park, its eastern boundary is the Luangwa River, while it rises to cover a stretch of the Muchinga Escarpment to the west. The Mwaleshi River flows east-west through the centre of the park, the area to its south being a strict wilderness zone.</obo:IAO_0000115>
        <oboInOwl:hasOBONamespace>GAZ</oboInOwl:hasOBONamespace>
        <oboInOwl:id>GAZ:00076747</oboInOwl:id>
        <rdfs:label>North Luangwa National Park</rdfs:label>
    </owl:NamedIndividual>
    


    <!-- http://purl.obolibrary.org/obo/GAZ_00076748 -->

    <owl:NamedIndividual rdf:about="http://purl.obolibrary.org/obo/GAZ_00076748">
        <obo:RO_0001025 rdf:resource="http://purl.obolibrary.org/obo/GAZ_00009430"/>
        <obo:IAO_0000115>A 5000 km2 park in the very south west corner of Zambia. The park occupies part of large plain lying between the Zambezi, the Cuando River (the upper Chobe River), and the Caprivi Strip, called the Silowana Plains, lying south of the Barotse Floodplain.</obo:IAO_0000115>
        <oboInOwl:hasOBONamespace>GAZ</oboInOwl:hasOBONamespace>
        <oboInOwl:id>GAZ:00076748</oboInOwl:id>
        <rdfs:label>Sioma Ngwezi National Park</rdfs:label>
    </owl:NamedIndividual>
    


    <!-- http://purl.obolibrary.org/obo/GAZ_00076749 -->

    <owl:NamedIndividual rdf:about="http://purl.obolibrary.org/obo/GAZ_00076749">
        <obo:RO_0001025 rdf:resource="http://purl.obolibrary.org/obo/GAZ_00009421"/>
        <obo:RO_0001025 rdf:resource="http://purl.obolibrary.org/obo/GAZ_00009423"/>
        <obo:RO_0001025 rdf:resource="http://purl.obolibrary.org/obo/GAZ_00009429"/>
        <obo:IAO_0000115>A national park in eastern Zambia, the southernmost of three national parks in the valley of the Luangwa River. The Muchinga Escarpment in Northern and Central Provinces forms the park&apos;s western or north-western boundary, it slopes down from there to the river, lying mostly on its western bank. Founded as a game reserve in 1938, it became a national park in 1972.</obo:IAO_0000115>
        <oboInOwl:hasOBONamespace>GAZ</oboInOwl:hasOBONamespace>
        <oboInOwl:id>GAZ:00076749</oboInOwl:id>
        <rdfs:label>South Luangwa National Park</rdfs:label>
    </owl:NamedIndividual>
    


    <!-- http://purl.obolibrary.org/obo/GAZ_00076750 -->

    <owl:NamedIndividual rdf:about="http://purl.obolibrary.org/obo/GAZ_00076750">
        <obo:RO_0001025 rdf:resource="http://purl.obolibrary.org/obo/GAZ_00009428"/>
        <obo:IAO_0000115>A national park in dense forest in the North-Western Province of Zambia. It lies between the West Lunga and Kabompo Rivers about 10 km north of the gravel road from Solwezi to Kabompo, and covers about 1700 km2.</obo:IAO_0000115>
        <oboInOwl:hasOBONamespace>GAZ</oboInOwl:hasOBONamespace>
        <oboInOwl:id>GAZ:00076750</oboInOwl:id>
        <rdfs:label>West Lunga National Park</rdfs:label>
    </owl:NamedIndividual>
    


    <!-- http://purl.obolibrary.org/obo/GAZ_00076754 -->

    <owl:NamedIndividual rdf:about="http://purl.obolibrary.org/obo/GAZ_00076754">
        <obo:IAO_0000115>A wildlife conservation area in Western Zimbabwe constituting a National Park. It is a region of the lower Zambezi River in Zimbabwe where the flood plain turns into a broad expanse of lakes after each rainy season. A World Heritage Site.</obo:IAO_0000115>
        <oboInOwl:hasOBONamespace>GAZ</oboInOwl:hasOBONamespace>
        <oboInOwl:id>GAZ:00076754</oboInOwl:id>
        <rdfs:label>Mana Pools National Park</rdfs:label>
    </owl:NamedIndividual>
    


    <!-- http://purl.obolibrary.org/obo/GAZ_00135241 -->

    <owl:NamedIndividual rdf:about="http://purl.obolibrary.org/obo/GAZ_00135241">
        <obo:IAO_0000115>A dam on the Mazoe River in Zimbabwe, north of Harare. It was built mainly to provide irrigation for the Mazoe citrus estates. Constructed 1920.</obo:IAO_0000115>
        <oboInOwl:hasOBONamespace>GAZ</oboInOwl:hasOBONamespace>
        <oboInOwl:id>GAZ:00135241</oboInOwl:id>
        <rdfs:label>Mazoe Dam</rdfs:label>
    </owl:NamedIndividual>
    


    <!-- http://purl.obolibrary.org/obo/GAZ_00136227 -->

    <owl:NamedIndividual rdf:about="http://purl.obolibrary.org/obo/GAZ_00136227">
        <obo:RO_0001025 rdf:resource="http://purl.obolibrary.org/obo/GAZ_00009429"/>
        <obo:IAO_0000115>A major wetland in the Central Province of Zambia, about 50 km west of Kabwe. It is permanently swampy area consists of a roughly circular area with a diameter of 40 to 50 km covering 1850 km2, plus roughly 250 km2 in the mouths of and along rivers discharging into it such as the Lukanga River from the north-east, plus another 500 km2 either side of the Kafue River to the west and north-west, making 2600 km2 in total. It contains many lagoons such as Lake Chiposhye and Lake Suye but few large channels, and its average depth is only 1.5 m.</obo:IAO_0000115>
        <oboInOwl:hasOBONamespace>GAZ</oboInOwl:hasOBONamespace>
        <oboInOwl:id>GAZ:00136227</oboInOwl:id>
        <rdfs:label>Lukanga Swamp</rdfs:label>
    </owl:NamedIndividual>
    


    <!-- http://purl.obolibrary.org/obo/GAZ_00136228 -->

    <owl:NamedIndividual rdf:about="http://purl.obolibrary.org/obo/GAZ_00136228">
        <obo:RO_0001025 rdf:resource="http://purl.obolibrary.org/obo/GAZ_00136227"/>
        <obo:IAO_0000115>A lake.</obo:IAO_0000115>
        <oboInOwl:hasOBONamespace>GAZ</oboInOwl:hasOBONamespace>
        <oboInOwl:id>GAZ:00136228</oboInOwl:id>
        <rdfs:label>Lake Chiposhye</rdfs:label>
    </owl:NamedIndividual>
    


    <!-- http://purl.obolibrary.org/obo/GAZ_00136229 -->

    <owl:NamedIndividual rdf:about="http://purl.obolibrary.org/obo/GAZ_00136229">
        <obo:RO_0001025 rdf:resource="http://purl.obolibrary.org/obo/GAZ_00136227"/>
        <obo:IAO_0000115>A lake.</obo:IAO_0000115>
        <oboInOwl:hasOBONamespace>GAZ</oboInOwl:hasOBONamespace>
        <oboInOwl:id>GAZ:00136229</oboInOwl:id>
        <rdfs:label>Lake Suye</rdfs:label>
    </owl:NamedIndividual>
    


    <!-- http://purl.obolibrary.org/obo/GAZ_00136230 -->

    <owl:NamedIndividual rdf:about="http://purl.obolibrary.org/obo/GAZ_00136230">
        <obo:RO_0001025 rdf:resource="http://purl.obolibrary.org/obo/GAZ_00136227"/>
        <obo:IAO_0000115>An island in Lukanga Swamp.</obo:IAO_0000115>
        <oboInOwl:hasOBONamespace>GAZ</oboInOwl:hasOBONamespace>
        <oboInOwl:id>GAZ:00136230</oboInOwl:id>
        <rdfs:label>Chilwa Island</rdfs:label>
    </owl:NamedIndividual>
    


    <!-- http://purl.obolibrary.org/obo/GAZ_00136231 -->

    <owl:NamedIndividual rdf:about="http://purl.obolibrary.org/obo/GAZ_00136231">
        <obo:RO_0001025 rdf:resource="http://purl.obolibrary.org/obo/GAZ_00136227"/>
        <obo:IAO_0000115>An island in Lukanga Swamp.</obo:IAO_0000115>
        <oboInOwl:hasOBONamespace>GAZ</oboInOwl:hasOBONamespace>
        <oboInOwl:id>GAZ:00136231</oboInOwl:id>
        <rdfs:label>Chiposha Island</rdfs:label>
    </owl:NamedIndividual>
    


    <!-- http://purl.obolibrary.org/obo/GAZ_00136232 -->

    <owl:NamedIndividual rdf:about="http://purl.obolibrary.org/obo/GAZ_00136232">
        <obo:RO_0001025 rdf:resource="http://purl.obolibrary.org/obo/GAZ_00015144"/>
        <obo:IAO_0000115>A protected area W of Kitwe.</obo:IAO_0000115>
        <oboInOwl:hasOBONamespace>GAZ</oboInOwl:hasOBONamespace>
        <oboInOwl:id>GAZ:00136232</oboInOwl:id>
        <rdfs:label>Chembe Bird Sanctuary</rdfs:label>
    </owl:NamedIndividual>
    


    <!-- http://purl.obolibrary.org/obo/GAZ_00136233 -->

    <owl:NamedIndividual rdf:about="http://purl.obolibrary.org/obo/GAZ_00136233">
        <obo:RO_0001025 rdf:resource="http://purl.obolibrary.org/obo/GAZ_00015182"/>
        <obo:RO_0001025 rdf:resource="http://purl.obolibrary.org/obo/GAZ_00049226"/>
        <obo:IAO_0000115>An island in Lake Bangweulu.</obo:IAO_0000115>
        <oboInOwl:hasOBONamespace>GAZ</oboInOwl:hasOBONamespace>
        <oboInOwl:id>GAZ:00136233</oboInOwl:id>
        <rdfs:label>Chichile Island</rdfs:label>
    </owl:NamedIndividual>
    


    <!-- http://purl.obolibrary.org/obo/GAZ_00136234 -->

    <owl:NamedIndividual rdf:about="http://purl.obolibrary.org/obo/GAZ_00136234">
        <obo:RO_0001025 rdf:resource="http://purl.obolibrary.org/obo/GAZ_00015182"/>
        <obo:RO_0001025 rdf:resource="http://purl.obolibrary.org/obo/GAZ_00049226"/>
        <obo:IAO_0000115>An island in Lake Bangweulu.</obo:IAO_0000115>
        <oboInOwl:hasOBONamespace>GAZ</oboInOwl:hasOBONamespace>
        <oboInOwl:id>GAZ:00136234</oboInOwl:id>
        <rdfs:label>Luangwa Island</rdfs:label>
    </owl:NamedIndividual>
    


    <!-- http://purl.obolibrary.org/obo/GAZ_00136235 -->

    <owl:NamedIndividual rdf:about="http://purl.obolibrary.org/obo/GAZ_00136235">
        <obo:RO_0001025 rdf:resource="http://purl.obolibrary.org/obo/GAZ_00015182"/>
        <obo:RO_0001025 rdf:resource="http://purl.obolibrary.org/obo/GAZ_00049226"/>
        <obo:IAO_0000115>An island in Lake Bangweulu.</obo:IAO_0000115>
        <oboInOwl:hasOBONamespace>GAZ</oboInOwl:hasOBONamespace>
        <oboInOwl:id>GAZ:00136235</oboInOwl:id>
        <rdfs:label>Kasansa Island</rdfs:label>
    </owl:NamedIndividual>
    


    <!-- http://purl.obolibrary.org/obo/GAZ_00136236 -->

    <owl:NamedIndividual rdf:about="http://purl.obolibrary.org/obo/GAZ_00136236">
        <obo:RO_0001025 rdf:resource="http://purl.obolibrary.org/obo/GAZ_00015182"/>
        <obo:RO_0001025 rdf:resource="http://purl.obolibrary.org/obo/GAZ_00049226"/>
        <obo:IAO_0000115>An island in Lake Bangweulu.</obo:IAO_0000115>
        <oboInOwl:hasOBONamespace>GAZ</oboInOwl:hasOBONamespace>
        <oboInOwl:id>GAZ:00136236</oboInOwl:id>
        <rdfs:label>Panyo Island</rdfs:label>
    </owl:NamedIndividual>
    


    <!-- http://purl.obolibrary.org/obo/GAZ_00234085 -->

    <owl:NamedIndividual rdf:about="http://purl.obolibrary.org/obo/GAZ_00234085">
        <obo:IAO_0000115>A hydroelectric dam. Located at the Ruzizi River outlet from Lake Kivu. Constructed 1958.</obo:IAO_0000115>
        <oboInOwl:hasOBONamespace>GAZ</oboInOwl:hasOBONamespace>
        <oboInOwl:id>GAZ:00234085</oboInOwl:id>
        <rdfs:label>Ruzizi I Hydroelectric Dam</rdfs:label>
    </owl:NamedIndividual>
    


    <!-- http://purl.obolibrary.org/obo/GAZ_00236226 -->

    <owl:NamedIndividual rdf:about="http://purl.obolibrary.org/obo/GAZ_00236226">
        <obo:IAO_0000115>An embankment dam with a hydroelectric power station and man-made lake near Kabwe, Zambia. Constructed 1950s.</obo:IAO_0000115>
        <oboInOwl:hasOBONamespace>GAZ</oboInOwl:hasOBONamespace>
        <oboInOwl:id>GAZ:00236226</oboInOwl:id>
        <rdfs:label>Mita Hills Dam</rdfs:label>
    </owl:NamedIndividual>
    


    <!-- http://purl.obolibrary.org/obo/GAZ_00236228 -->

    <owl:NamedIndividual rdf:about="http://purl.obolibrary.org/obo/GAZ_00236228">
        <obo:IAO_0000115>A lake.</obo:IAO_0000115>
        <oboInOwl:hasOBONamespace>GAZ</oboInOwl:hasOBONamespace>
        <oboInOwl:id>GAZ:00236228</oboInOwl:id>
        <rdfs:label>Lake Kazuni</rdfs:label>
    </owl:NamedIndividual>
    


    <!-- http://purl.obolibrary.org/obo/GAZ_00236229 -->

    <owl:NamedIndividual rdf:about="http://purl.obolibrary.org/obo/GAZ_00236229">
        <obo:RO_0001025 rdf:resource="http://purl.obolibrary.org/obo/GAZ_00076592"/>
        <obo:IAO_0000115>A lake of Malawi. It is 8 km west of Chisti and is located inside Nyika National Park.</obo:IAO_0000115>
        <oboInOwl:hasOBONamespace>GAZ</oboInOwl:hasOBONamespace>
        <oboInOwl:id>GAZ:00236229</oboInOwl:id>
        <rdfs:label>Lake Kaulime</rdfs:label>
    </owl:NamedIndividual>
    


    <!-- http://purl.obolibrary.org/obo/GAZ_00237419 -->

    <owl:NamedIndividual rdf:about="http://purl.obolibrary.org/obo/GAZ_00237419">
        <obo:RO_0001025 rdf:resource="http://purl.obolibrary.org/obo/GAZ_00009428"/>
        <obo:IAO_0000115>A river.</obo:IAO_0000115>
        <oboInOwl:hasOBONamespace>GAZ</oboInOwl:hasOBONamespace>
        <oboInOwl:id>GAZ:00237419</oboInOwl:id>
        <rdfs:label>Western Lunga River</rdfs:label>
    </owl:NamedIndividual>
    


    <!-- http://purl.obolibrary.org/obo/GAZ_00237423 -->

    <owl:NamedIndividual rdf:about="http://purl.obolibrary.org/obo/GAZ_00237423">
        <obo:IAO_0000115>A wetland. Located E of Lukulu on the Luena River immediately before it leaves the plateau proper and enters the Zambezi Valley.</obo:IAO_0000115>
        <oboInOwl:hasOBONamespace>GAZ</oboInOwl:hasOBONamespace>
        <oboInOwl:id>GAZ:00237423</oboInOwl:id>
        <rdfs:label>Luena Flats</rdfs:label>
    </owl:NamedIndividual>
    


    <!-- http://purl.obolibrary.org/obo/GAZ_00237429 -->

    <owl:NamedIndividual rdf:about="http://purl.obolibrary.org/obo/GAZ_00237429">
        <obo:RO_0001025 rdf:resource="http://purl.obolibrary.org/obo/GAZ_00016178"/>
        <obo:IAO_0000115>An island in Lake Kariba.</obo:IAO_0000115>
        <oboInOwl:hasOBONamespace>GAZ</oboInOwl:hasOBONamespace>
        <oboInOwl:id>GAZ:00237429</oboInOwl:id>
        <rdfs:label>Maaze Island</rdfs:label>
    </owl:NamedIndividual>
    


    <!-- http://purl.obolibrary.org/obo/GAZ_00237430 -->

    <owl:NamedIndividual rdf:about="http://purl.obolibrary.org/obo/GAZ_00237430">
        <obo:RO_0001025 rdf:resource="http://purl.obolibrary.org/obo/GAZ_00016178"/>
        <obo:IAO_0000115>An island in Lake Kariba.</obo:IAO_0000115>
        <oboInOwl:hasOBONamespace>GAZ</oboInOwl:hasOBONamespace>
        <oboInOwl:id>GAZ:00237430</oboInOwl:id>
        <rdfs:label>Mashape Island</rdfs:label>
    </owl:NamedIndividual>
    


    <!-- http://purl.obolibrary.org/obo/GAZ_00237431 -->

    <owl:NamedIndividual rdf:about="http://purl.obolibrary.org/obo/GAZ_00237431">
        <obo:RO_0001025 rdf:resource="http://purl.obolibrary.org/obo/GAZ_00016178"/>
        <obo:IAO_0000115>An island in Lake Kariba.</obo:IAO_0000115>
        <oboInOwl:hasOBONamespace>GAZ</oboInOwl:hasOBONamespace>
        <oboInOwl:id>GAZ:00237431</oboInOwl:id>
        <rdfs:label>Sampa Karuma Island</rdfs:label>
    </owl:NamedIndividual>
    


    <!-- http://purl.obolibrary.org/obo/GAZ_00237432 -->

    <owl:NamedIndividual rdf:about="http://purl.obolibrary.org/obo/GAZ_00237432">
        <obo:RO_0001025 rdf:resource="http://purl.obolibrary.org/obo/GAZ_00016178"/>
        <obo:IAO_0000115>An island in Lake Kariba.</obo:IAO_0000115>
        <oboInOwl:hasOBONamespace>GAZ</oboInOwl:hasOBONamespace>
        <oboInOwl:id>GAZ:00237432</oboInOwl:id>
        <rdfs:label>Fothergill Island</rdfs:label>
    </owl:NamedIndividual>
    


    <!-- http://purl.obolibrary.org/obo/GAZ_00237433 -->

    <owl:NamedIndividual rdf:about="http://purl.obolibrary.org/obo/GAZ_00237433">
        <obo:RO_0001025 rdf:resource="http://purl.obolibrary.org/obo/GAZ_00016178"/>
        <obo:IAO_0000115>An island in Lake Kariba.</obo:IAO_0000115>
        <oboInOwl:hasOBONamespace>GAZ</oboInOwl:hasOBONamespace>
        <oboInOwl:id>GAZ:00237433</oboInOwl:id>
        <rdfs:label>Spurwing Island</rdfs:label>
    </owl:NamedIndividual>
    


    <!-- http://purl.obolibrary.org/obo/GAZ_00237434 -->

    <owl:NamedIndividual rdf:about="http://purl.obolibrary.org/obo/GAZ_00237434">
        <obo:RO_0001025 rdf:resource="http://purl.obolibrary.org/obo/GAZ_00016178"/>
        <obo:IAO_0000115>An island in Lake Kariba.</obo:IAO_0000115>
        <oboInOwl:hasOBONamespace>GAZ</oboInOwl:hasOBONamespace>
        <oboInOwl:id>GAZ:00237434</oboInOwl:id>
        <rdfs:label>Snake Island</rdfs:label>
    </owl:NamedIndividual>
    


    <!-- http://purl.obolibrary.org/obo/GAZ_00237435 -->

    <owl:NamedIndividual rdf:about="http://purl.obolibrary.org/obo/GAZ_00237435">
        <obo:RO_0001025 rdf:resource="http://purl.obolibrary.org/obo/GAZ_00016178"/>
        <obo:IAO_0000115>An island in Lake Kariba.</obo:IAO_0000115>
        <oboInOwl:hasOBONamespace>GAZ</oboInOwl:hasOBONamespace>
        <oboInOwl:id>GAZ:00237435</oboInOwl:id>
        <rdfs:label>Antelope Island</rdfs:label>
    </owl:NamedIndividual>
    


    <!-- http://purl.obolibrary.org/obo/GAZ_00237436 -->

    <owl:NamedIndividual rdf:about="http://purl.obolibrary.org/obo/GAZ_00237436">
        <obo:RO_0001025 rdf:resource="http://purl.obolibrary.org/obo/GAZ_00016178"/>
        <obo:IAO_0000115>An island in Lake Kariba.</obo:IAO_0000115>
        <oboInOwl:hasOBONamespace>GAZ</oboInOwl:hasOBONamespace>
        <oboInOwl:id>GAZ:00237436</oboInOwl:id>
        <rdfs:label>Bed Island</rdfs:label>
    </owl:NamedIndividual>
    


    <!-- http://purl.obolibrary.org/obo/GAZ_00237437 -->

    <owl:NamedIndividual rdf:about="http://purl.obolibrary.org/obo/GAZ_00237437">
        <obo:RO_0001025 rdf:resource="http://purl.obolibrary.org/obo/GAZ_00016178"/>
        <obo:IAO_0000115>An island in Lake Kariba.</obo:IAO_0000115>
        <oboInOwl:hasOBONamespace>GAZ</oboInOwl:hasOBONamespace>
        <oboInOwl:id>GAZ:00237437</oboInOwl:id>
        <rdfs:label>Chikanka Island</rdfs:label>
    </owl:NamedIndividual>
    


    <!-- http://purl.obolibrary.org/obo/GAZ_00237440 -->

    <owl:NamedIndividual rdf:about="http://purl.obolibrary.org/obo/GAZ_00237440">
        <obo:RO_0001025 rdf:resource="http://purl.obolibrary.org/obo/GAZ_00009428"/>
        <obo:IAO_0000115>A river. A tributary of the Kafue River.</obo:IAO_0000115>
        <oboInOwl:hasOBONamespace>GAZ</oboInOwl:hasOBONamespace>
        <oboInOwl:id>GAZ:00237440</oboInOwl:id>
        <rdfs:label>Lunga River</rdfs:label>
    </owl:NamedIndividual>
    


    <!-- http://purl.obolibrary.org/obo/GAZ_00237443 -->

    <owl:NamedIndividual rdf:about="http://purl.obolibrary.org/obo/GAZ_00237443">
        <obo:IAO_0000115>A dam. Constructed 1972.</obo:IAO_0000115>
        <oboInOwl:hasOBONamespace>GAZ</oboInOwl:hasOBONamespace>
        <oboInOwl:id>GAZ:00237443</oboInOwl:id>
        <rdfs:label>Kafue Gorge Dam</rdfs:label>
    </owl:NamedIndividual>
    


    <!-- http://purl.obolibrary.org/obo/GAZ_00237444 -->

    <owl:NamedIndividual rdf:about="http://purl.obolibrary.org/obo/GAZ_00237444">
        <obo:RO_0001025 rdf:resource="http://purl.obolibrary.org/obo/GAZ_00015195"/>
        <obo:IAO_0000115>A protected are NE of the town of Choma.</obo:IAO_0000115>
        <oboInOwl:hasOBONamespace>GAZ</oboInOwl:hasOBONamespace>
        <oboInOwl:id>GAZ:00237444</oboInOwl:id>
        <rdfs:label>Nkanga River Conservation Area</rdfs:label>
    </owl:NamedIndividual>
    


    <!-- http://purl.obolibrary.org/obo/GAZ_00237445 -->

    <owl:NamedIndividual rdf:about="http://purl.obolibrary.org/obo/GAZ_00237445">
        <obo:IAO_0000115>A protected area.</obo:IAO_0000115>
        <oboInOwl:hasOBONamespace>GAZ</oboInOwl:hasOBONamespace>
        <oboInOwl:id>GAZ:00237445</oboInOwl:id>
        <rdfs:label>Mwanachingwala Conservation Area</rdfs:label>
    </owl:NamedIndividual>
    


    <!-- http://purl.obolibrary.org/obo/GAZ_00237446 -->

    <owl:NamedIndividual rdf:about="http://purl.obolibrary.org/obo/GAZ_00237446">
        <obo:IAO_0000115>A lake.</obo:IAO_0000115>
        <oboInOwl:hasOBONamespace>GAZ</oboInOwl:hasOBONamespace>
        <oboInOwl:id>GAZ:00237446</oboInOwl:id>
        <rdfs:label>Lake Kampolombo</rdfs:label>
    </owl:NamedIndividual>
    


    <!-- http://purl.obolibrary.org/obo/GAZ_00237447 -->

    <owl:NamedIndividual rdf:about="http://purl.obolibrary.org/obo/GAZ_00237447">
        <obo:IAO_0000115>A lake.</obo:IAO_0000115>
        <oboInOwl:hasOBONamespace>GAZ</oboInOwl:hasOBONamespace>
        <oboInOwl:id>GAZ:00237447</oboInOwl:id>
        <rdfs:label>Lake Chifungwe</rdfs:label>
    </owl:NamedIndividual>
    


    <!-- http://purl.obolibrary.org/obo/GAZ_00237449 -->

    <owl:NamedIndividual rdf:about="http://purl.obolibrary.org/obo/GAZ_00237449">
        <obo:RO_0001025 rdf:resource="http://purl.obolibrary.org/obo/GAZ_00009423"/>
        <obo:IAO_0000115>A river.</obo:IAO_0000115>
        <oboInOwl:hasOBONamespace>GAZ</oboInOwl:hasOBONamespace>
        <oboInOwl:id>GAZ:00237449</oboInOwl:id>
        <rdfs:label>Lufubu River</rdfs:label>
    </owl:NamedIndividual>
    


    <!-- http://purl.obolibrary.org/obo/GAZ_00237450 -->

    <owl:NamedIndividual rdf:about="http://purl.obolibrary.org/obo/GAZ_00237450">
        <obo:RO_0001025 rdf:resource="http://purl.obolibrary.org/obo/GAZ_00015172"/>
        <obo:IAO_0000115>A river.</obo:IAO_0000115>
        <oboInOwl:hasOBONamespace>GAZ</oboInOwl:hasOBONamespace>
        <oboInOwl:id>GAZ:00237450</oboInOwl:id>
        <rdfs:label>West Lunga River</rdfs:label>
    </owl:NamedIndividual>
    


    <!-- http://purl.obolibrary.org/obo/GAZ_00237451 -->

    <owl:NamedIndividual rdf:about="http://purl.obolibrary.org/obo/GAZ_00237451">
        <obo:RO_0001025 rdf:resource="http://purl.obolibrary.org/obo/GAZ_00015172"/>
        <obo:IAO_0000115>A protected area.</obo:IAO_0000115>
        <oboInOwl:hasOBONamespace>GAZ</oboInOwl:hasOBONamespace>
        <oboInOwl:id>GAZ:00237451</oboInOwl:id>
        <rdfs:label>Nchila Wildlife Reserve</rdfs:label>
    </owl:NamedIndividual>
    


    <!-- http://purl.obolibrary.org/obo/GAZ_00237452 -->

    <owl:NamedIndividual rdf:about="http://purl.obolibrary.org/obo/GAZ_00237452">
        <obo:RO_0001025 rdf:resource="http://purl.obolibrary.org/obo/GAZ_00015172"/>
        <obo:IAO_0000115>A protected area.</obo:IAO_0000115>
        <oboInOwl:hasOBONamespace>GAZ</oboInOwl:hasOBONamespace>
        <oboInOwl:id>GAZ:00237452</oboInOwl:id>
        <rdfs:label>Luakela Forest Reserve</rdfs:label>
    </owl:NamedIndividual>
    


    <!-- http://purl.obolibrary.org/obo/GAZ_00237454 -->

    <owl:NamedIndividual rdf:about="http://purl.obolibrary.org/obo/GAZ_00237454">
        <obo:RO_0001025 rdf:resource="http://purl.obolibrary.org/obo/GAZ_00015162"/>
        <obo:IAO_0000115>A river.</obo:IAO_0000115>
        <oboInOwl:hasOBONamespace>GAZ</oboInOwl:hasOBONamespace>
        <oboInOwl:id>GAZ:00237454</oboInOwl:id>
        <rdfs:label>Lwela River</rdfs:label>
    </owl:NamedIndividual>
    


    <!-- http://purl.obolibrary.org/obo/GAZ_00237455 -->

    <owl:NamedIndividual rdf:about="http://purl.obolibrary.org/obo/GAZ_00237455">
        <obo:RO_0001025 rdf:resource="http://purl.obolibrary.org/obo/GAZ_00015141"/>
        <obo:IAO_0000115>A lake. Located 14 km E of Ndola. It was formed by the collapse of rock into an underlying limestone cavern.</obo:IAO_0000115>
        <oboInOwl:hasOBONamespace>GAZ</oboInOwl:hasOBONamespace>
        <oboInOwl:id>GAZ:00237455</oboInOwl:id>
        <rdfs:label>Lake Chilengwa</rdfs:label>
    </owl:NamedIndividual>
    


    <!-- http://purl.obolibrary.org/obo/GAZ_00237456 -->

    <owl:NamedIndividual rdf:about="http://purl.obolibrary.org/obo/GAZ_00237456">
        <obo:RO_0001025 rdf:resource="http://purl.obolibrary.org/obo/GAZ_00015146"/>
        <obo:IAO_0000115>A river.</obo:IAO_0000115>
        <oboInOwl:hasOBONamespace>GAZ</oboInOwl:hasOBONamespace>
        <oboInOwl:id>GAZ:00237456</oboInOwl:id>
        <rdfs:label>Luanshya River</rdfs:label>
    </owl:NamedIndividual>
    


    <!-- http://purl.obolibrary.org/obo/GAZ_00237457 -->

    <owl:NamedIndividual rdf:about="http://purl.obolibrary.org/obo/GAZ_00237457">
        <obo:RO_0001025 rdf:resource="http://purl.obolibrary.org/obo/GAZ_00015142"/>
        <obo:IAO_0000115>A protected area.</obo:IAO_0000115>
        <oboInOwl:hasOBONamespace>GAZ</oboInOwl:hasOBONamespace>
        <oboInOwl:id>GAZ:00237457</oboInOwl:id>
        <rdfs:label>Chati Forest Reserve</rdfs:label>
    </owl:NamedIndividual>
    


    <!-- http://purl.obolibrary.org/obo/GAZ_00237458 -->

    <owl:NamedIndividual rdf:about="http://purl.obolibrary.org/obo/GAZ_00237458">
        <obo:RO_0001025 rdf:resource="http://purl.obolibrary.org/obo/GAZ_00015148"/>
        <obo:IAO_0000115>Open copper ore mines that are situated in a crescent shaped structure 11 km long around the municipal town of Chingola in Zambia.</obo:IAO_0000115>
        <oboInOwl:hasOBONamespace>GAZ</oboInOwl:hasOBONamespace>
        <oboInOwl:id>GAZ:00237458</oboInOwl:id>
        <rdfs:label>Nchanga Open Pit Mine</rdfs:label>
    </owl:NamedIndividual>
    


    <!-- http://purl.obolibrary.org/obo/GAZ_00237459 -->

    <owl:NamedIndividual rdf:about="http://purl.obolibrary.org/obo/GAZ_00237459">
        <obo:RO_0001025 rdf:resource="http://purl.obolibrary.org/obo/GAZ_00015137"/>
        <obo:IAO_0000115>A populated place. The capital of the Zambian Central Province.</obo:IAO_0000115>
        <oboInOwl:hasOBONamespace>GAZ</oboInOwl:hasOBONamespace>
        <oboInOwl:id>GAZ:00237459</oboInOwl:id>
        <rdfs:label>Kabwe</rdfs:label>
    </owl:NamedIndividual>
    


    <!-- http://purl.obolibrary.org/obo/GAZ_00237460 -->

    <owl:NamedIndividual rdf:about="http://purl.obolibrary.org/obo/GAZ_00237460">
        <obo:RO_0001025 rdf:resource="http://purl.obolibrary.org/obo/GAZ_00058785"/>
        <obo:IAO_0000115>A dam. Impounds Mulungushi Reservoir. Completed 1925.</obo:IAO_0000115>
        <oboInOwl:hasOBONamespace>GAZ</oboInOwl:hasOBONamespace>
        <oboInOwl:id>GAZ:00237460</oboInOwl:id>
        <rdfs:label>Mulungushi Dam</rdfs:label>
    </owl:NamedIndividual>
    


    <!-- http://purl.obolibrary.org/obo/GAZ_00237461 -->

    <owl:NamedIndividual rdf:about="http://purl.obolibrary.org/obo/GAZ_00237461">
        <obo:RO_0001025 rdf:resource="http://purl.obolibrary.org/obo/GAZ_00009429"/>
        <obo:IAO_0000115>Mountains 50 km east of Kabwe. A wilderness area of rugged granite mountains rising 1000 m above the Luangwa Valley, just to the north-west of the confluence of the Lunsemfwa and Lukusashi Rivers.</obo:IAO_0000115>
        <oboInOwl:hasOBONamespace>GAZ</oboInOwl:hasOBONamespace>
        <oboInOwl:id>GAZ:00237461</oboInOwl:id>
        <rdfs:label>Chifunkunya Hills</rdfs:label>
    </owl:NamedIndividual>
    


    <!-- http://purl.obolibrary.org/obo/GAZ_00237650 -->

    <owl:NamedIndividual rdf:about="http://purl.obolibrary.org/obo/GAZ_00237650">
        <obo:IAO_0000115>A dam.</obo:IAO_0000115>
        <oboInOwl:hasOBONamespace>GAZ</oboInOwl:hasOBONamespace>
        <oboInOwl:id>GAZ:00237650</oboInOwl:id>
        <rdfs:label>Ngezi Dam</rdfs:label>
    </owl:NamedIndividual>
    


    <!-- http://purl.obolibrary.org/obo/GAZ_00237862 -->

    <owl:NamedIndividual rdf:about="http://purl.obolibrary.org/obo/GAZ_00237862">
        <obo:IAO_0000115>A river.</obo:IAO_0000115>
        <oboInOwl:hasOBONamespace>GAZ</oboInOwl:hasOBONamespace>
        <oboInOwl:id>GAZ:00237862</oboInOwl:id>
        <rdfs:label>Utembo River</rdfs:label>
    </owl:NamedIndividual>
    


    <!-- http://purl.obolibrary.org/obo/GAZ_00238896 -->

    <owl:NamedIndividual rdf:about="http://purl.obolibrary.org/obo/GAZ_00238896">
        <obo:IAO_0000115>An island in the Chobe River on the border between Namibia and Botswana, near the Botswanan town of Kasane. It was the subject of a territorial dispute between these countries, resolved by a 1999 decision of the International Court of Justice which ruled in favour of Botswana.</obo:IAO_0000115>
        <oboInOwl:hasOBONamespace>GAZ</oboInOwl:hasOBONamespace>
        <oboInOwl:id>GAZ:00238896</oboInOwl:id>
        <rdfs:label>Kasikili Island</rdfs:label>
    </owl:NamedIndividual>
    


    <!-- http://purl.obolibrary.org/obo/GAZ_00239433 -->

    <owl:NamedIndividual rdf:about="http://purl.obolibrary.org/obo/GAZ_00239433">
        <obo:IAO_0000115>An island.</obo:IAO_0000115>
        <oboInOwl:hasOBONamespace>GAZ</oboInOwl:hasOBONamespace>
        <oboInOwl:id>GAZ:00239433</oboInOwl:id>
        <rdfs:label>Nkasa Island</rdfs:label>
    </owl:NamedIndividual>
    


    <!-- http://purl.obolibrary.org/obo/GAZ_00239434 -->

    <owl:NamedIndividual rdf:about="http://purl.obolibrary.org/obo/GAZ_00239434">
        <obo:IAO_0000115>An island.</obo:IAO_0000115>
        <oboInOwl:hasOBONamespace>GAZ</oboInOwl:hasOBONamespace>
        <oboInOwl:id>GAZ:00239434</oboInOwl:id>
        <rdfs:label>Lupala island</rdfs:label>
    </owl:NamedIndividual>
    


    <!-- http://purl.obolibrary.org/obo/GAZ_00239437 -->

    <owl:NamedIndividual rdf:about="http://purl.obolibrary.org/obo/GAZ_00239437">
        <obo:IAO_0000115>A freshwater lake. A wide part of the Cuando River.</obo:IAO_0000115>
        <oboInOwl:hasOBONamespace>GAZ</oboInOwl:hasOBONamespace>
        <oboInOwl:id>GAZ:00239437</oboInOwl:id>
        <rdfs:label>Liambezi Lake</rdfs:label>
    </owl:NamedIndividual>
    


    <!-- http://purl.obolibrary.org/obo/GAZ_00247094 -->

    <owl:NamedIndividual rdf:about="http://purl.obolibrary.org/obo/GAZ_00247094">
        <obo:IAO_0000115>A river that flows into Lake Tanganyika in the south of Burundi.</obo:IAO_0000115>
        <oboInOwl:hasOBONamespace>GAZ</oboInOwl:hasOBONamespace>
        <oboInOwl:id>GAZ:00247094</oboInOwl:id>
        <rdfs:label>Mugwezi River</rdfs:label>
    </owl:NamedIndividual>
    


    <!-- http://purl.obolibrary.org/obo/GAZ_00247095 -->

    <owl:NamedIndividual rdf:about="http://purl.obolibrary.org/obo/GAZ_00247095">
        <obo:IAO_0000115>A river that flows into Lake Tanganyika in the south of Burundi.</obo:IAO_0000115>
        <oboInOwl:hasOBONamespace>GAZ</oboInOwl:hasOBONamespace>
        <oboInOwl:id>GAZ:00247095</oboInOwl:id>
        <rdfs:label>Luaba River</rdfs:label>
    </owl:NamedIndividual>
    


    <!-- http://purl.obolibrary.org/obo/GAZ_00251886 -->

    <owl:NamedIndividual rdf:about="http://purl.obolibrary.org/obo/GAZ_00251886">
        <obo:IAO_0000115>A wetland. A swamp fringed widening of the South Rukuru River.</obo:IAO_0000115>
        <oboInOwl:hasOBONamespace>GAZ</oboInOwl:hasOBONamespace>
        <oboInOwl:id>GAZ:00251886</oboInOwl:id>
        <rdfs:label>Zaro Pool</rdfs:label>
    </owl:NamedIndividual>
    


    <!-- http://purl.obolibrary.org/obo/GAZ_00251903 -->

    <owl:NamedIndividual rdf:about="http://purl.obolibrary.org/obo/GAZ_00251903">
        <obo:IAO_0000115>A widening of the Shire River?</obo:IAO_0000115>
        <oboInOwl:hasOBONamespace>GAZ</oboInOwl:hasOBONamespace>
        <oboInOwl:id>GAZ:00251903</oboInOwl:id>
        <rdfs:label>Bangula Lagoon</rdfs:label>
    </owl:NamedIndividual>
    


    <!-- http://purl.obolibrary.org/obo/GAZ_00256741 -->

    <owl:NamedIndividual rdf:about="http://purl.obolibrary.org/obo/GAZ_00256741">
        <obo:IAO_0000115>A river.</obo:IAO_0000115>
        <oboInOwl:hasOBONamespace>GAZ</oboInOwl:hasOBONamespace>
        <oboInOwl:id>GAZ:00256741</oboInOwl:id>
        <rdfs:label>Ziuwe River</rdfs:label>
    </owl:NamedIndividual>
    


    <!-- http://purl.obolibrary.org/obo/GAZ_00256743 -->

    <owl:NamedIndividual rdf:about="http://purl.obolibrary.org/obo/GAZ_00256743">
        <obo:RO_0001025 rdf:resource="http://purl.obolibrary.org/obo/GAZ_00256741"/>
        <obo:IAO_0000115>A lake.</obo:IAO_0000115>
        <oboInOwl:hasOBONamespace>GAZ</oboInOwl:hasOBONamespace>
        <oboInOwl:id>GAZ:00256743</oboInOwl:id>
        <rdfs:label>Lake Sagara</rdfs:label>
    </owl:NamedIndividual>
    


    <!-- http://purl.obolibrary.org/obo/GAZ_00260937 -->

    <owl:NamedIndividual rdf:about="http://purl.obolibrary.org/obo/GAZ_00260937">
        <obo:RO_0001025 rdf:resource="http://purl.obolibrary.org/obo/GAZ_00237423"/>
        <obo:IAO_0000115>A canal carrying water of the Luena River.</obo:IAO_0000115>
        <oboInOwl:hasOBONamespace>GAZ</oboInOwl:hasOBONamespace>
        <oboInOwl:id>GAZ:00260937</oboInOwl:id>
        <rdfs:label>Lubitanei Canal</rdfs:label>
    </owl:NamedIndividual>
    


    <!-- http://purl.obolibrary.org/obo/GAZ_00260940 -->

    <owl:NamedIndividual rdf:about="http://purl.obolibrary.org/obo/GAZ_00260940">
        <obo:IAO_0000115>A wetland. Located in the basin of the Luanginga, which joins the Zambezi near Lealui. The swamps are not on the Luanginga itself, but on and between some of its south bank tributaries, principally the Luate.</obo:IAO_0000115>
        <oboInOwl:hasOBONamespace>GAZ</oboInOwl:hasOBONamespace>
        <oboInOwl:id>GAZ:00260940</oboInOwl:id>
        <rdfs:label>Nyengo Swamps</rdfs:label>
    </owl:NamedIndividual>
    


    <!-- http://purl.obolibrary.org/obo/GAZ_00260941 -->

    <owl:NamedIndividual rdf:about="http://purl.obolibrary.org/obo/GAZ_00260941">
        <obo:IAO_0000115>A lake. Located on the plain to the south of the Nyengo Swamps.</obo:IAO_0000115>
        <oboInOwl:hasOBONamespace>GAZ</oboInOwl:hasOBONamespace>
        <oboInOwl:id>GAZ:00260941</oboInOwl:id>
        <rdfs:label>Lake Siliole</rdfs:label>
    </owl:NamedIndividual>
    


    <!-- http://purl.obolibrary.org/obo/GAZ_00260942 -->

    <owl:NamedIndividual rdf:about="http://purl.obolibrary.org/obo/GAZ_00260942">
        <obo:RO_0001025 rdf:resource="http://purl.obolibrary.org/obo/GAZ_00052642"/>
        <obo:IAO_0000115>A tributary which joins the Zambezi River just below Senanga on the Barotse Floodplain. It rises in Angola and drains the swampy southeastern interior of that country, including the Chiume Lakes.</obo:IAO_0000115>
        <oboInOwl:hasOBONamespace>GAZ</oboInOwl:hasOBONamespace>
        <oboInOwl:id>GAZ:00260942</oboInOwl:id>
        <rdfs:label>Lueti River</rdfs:label>
    </owl:NamedIndividual>
    


    <!-- http://purl.obolibrary.org/obo/GAZ_00260943 -->

    <owl:NamedIndividual rdf:about="http://purl.obolibrary.org/obo/GAZ_00260943">
        <obo:RO_0001025 rdf:resource="http://purl.obolibrary.org/obo/GAZ_00052642"/>
        <obo:IAO_0000115>A tributary which joins the Zambezi River just below Senanga on the Barotse Floodplain.</obo:IAO_0000115>
        <oboInOwl:hasOBONamespace>GAZ</oboInOwl:hasOBONamespace>
        <oboInOwl:id>GAZ:00260943</oboInOwl:id>
        <rdfs:label>Lui River</rdfs:label>
    </owl:NamedIndividual>
    


    <!-- http://purl.obolibrary.org/obo/GAZ_00260944 -->

    <owl:NamedIndividual rdf:about="http://purl.obolibrary.org/obo/GAZ_00260944">
        <obo:IAO_0000115>A wetland. A floodplain along the northern border of the Caprivi Strip.</obo:IAO_0000115>
        <oboInOwl:hasOBONamespace>GAZ</oboInOwl:hasOBONamespace>
        <oboInOwl:id>GAZ:00260944</oboInOwl:id>
        <rdfs:label>Sesheke-Maramba Floodplain</rdfs:label>
    </owl:NamedIndividual>
    


    <!-- http://purl.obolibrary.org/obo/GAZ_00260949 -->

    <owl:NamedIndividual rdf:about="http://purl.obolibrary.org/obo/GAZ_00260949">
        <obo:RO_0001025 rdf:resource="http://purl.obolibrary.org/obo/GAZ_00009428"/>
        <obo:IAO_0000115>A wetland.</obo:IAO_0000115>
        <oboInOwl:hasOBONamespace>GAZ</oboInOwl:hasOBONamespace>
        <oboInOwl:id>GAZ:00260949</oboInOwl:id>
        <rdfs:label>Busanga Swamp</rdfs:label>
    </owl:NamedIndividual>
    


    <!-- http://purl.obolibrary.org/obo/GAZ_00260950 -->

    <owl:NamedIndividual rdf:about="http://purl.obolibrary.org/obo/GAZ_00260950">
        <obo:RO_0001025 rdf:resource="http://purl.obolibrary.org/obo/GAZ_00009425"/>
        <obo:IAO_0000115>A wetland. Situated on the Lushwishi River above its confluence with the Mininga River.</obo:IAO_0000115>
        <oboInOwl:hasOBONamespace>GAZ</oboInOwl:hasOBONamespace>
        <oboInOwl:id>GAZ:00260950</oboInOwl:id>
        <rdfs:label>Lushwishi Swamp</rdfs:label>
    </owl:NamedIndividual>
    


    <!-- http://purl.obolibrary.org/obo/GAZ_00260952 -->

    <owl:NamedIndividual rdf:about="http://purl.obolibrary.org/obo/GAZ_00260952">
        <obo:RO_0001025 rdf:resource="http://purl.obolibrary.org/obo/GAZ_00009425"/>
        <obo:IAO_0000115>A wetland.</obo:IAO_0000115>
        <oboInOwl:hasOBONamespace>GAZ</oboInOwl:hasOBONamespace>
        <oboInOwl:id>GAZ:00260952</oboInOwl:id>
        <rdfs:label>Lufwanyama Swamp</rdfs:label>
    </owl:NamedIndividual>
    


    <!-- http://purl.obolibrary.org/obo/GAZ_00260953 -->

    <owl:NamedIndividual rdf:about="http://purl.obolibrary.org/obo/GAZ_00260953">
        <obo:RO_0001025 rdf:resource="http://purl.obolibrary.org/obo/GAZ_00009425"/>
        <obo:IAO_0000115>A wetland.</obo:IAO_0000115>
        <oboInOwl:hasOBONamespace>GAZ</oboInOwl:hasOBONamespace>
        <oboInOwl:id>GAZ:00260953</oboInOwl:id>
        <rdfs:label>Mininga Swamp</rdfs:label>
    </owl:NamedIndividual>
    


    <!-- http://purl.obolibrary.org/obo/GAZ_00260954 -->

    <owl:NamedIndividual rdf:about="http://purl.obolibrary.org/obo/GAZ_00260954">
        <obo:IAO_0000115>A lake.</obo:IAO_0000115>
        <oboInOwl:hasOBONamespace>GAZ</oboInOwl:hasOBONamespace>
        <oboInOwl:id>GAZ:00260954</oboInOwl:id>
        <rdfs:label>Lake Kangwena</rdfs:label>
    </owl:NamedIndividual>
    


    <!-- http://purl.obolibrary.org/obo/GAZ_00260957 -->

    <owl:NamedIndividual rdf:about="http://purl.obolibrary.org/obo/GAZ_00260957">
        <obo:RO_0001025 rdf:resource="http://purl.obolibrary.org/obo/GAZ_00009427"/>
        <obo:IAO_0000115>A wetland. Located S of Bangweulu Wetlands.</obo:IAO_0000115>
        <oboInOwl:hasOBONamespace>GAZ</oboInOwl:hasOBONamespace>
        <oboInOwl:id>GAZ:00260957</oboInOwl:id>
        <rdfs:label>Kapabi Swamps</rdfs:label>
    </owl:NamedIndividual>
    


    <!-- http://purl.obolibrary.org/obo/GAZ_00260963 -->

    <owl:NamedIndividual rdf:about="http://purl.obolibrary.org/obo/GAZ_00260963">
        <obo:RO_0001025 rdf:resource="http://purl.obolibrary.org/obo/GAZ_00041530"/>
        <obo:IAO_0000115>An island.</obo:IAO_0000115>
        <oboInOwl:hasOBONamespace>GAZ</oboInOwl:hasOBONamespace>
        <oboInOwl:id>GAZ:00260963</oboInOwl:id>
        <rdfs:label>N&apos;Kole Island</rdfs:label>
    </owl:NamedIndividual>
    


    <!-- http://purl.obolibrary.org/obo/GAZ_00260964 -->

    <owl:NamedIndividual rdf:about="http://purl.obolibrary.org/obo/GAZ_00260964">
        <obo:RO_0001025 rdf:resource="http://purl.obolibrary.org/obo/GAZ_00009427"/>
        <obo:RO_0001025 rdf:resource="http://purl.obolibrary.org/obo/GAZ_00058782"/>
        <obo:IAO_0000115>A lake lagoon in Zambia. It is in the Luapula River swamps south of Lake Mweru, in the Luapula Province of Zambia.</obo:IAO_0000115>
        <oboInOwl:hasOBONamespace>GAZ</oboInOwl:hasOBONamespace>
        <oboInOwl:id>GAZ:00260964</oboInOwl:id>
        <rdfs:label>Pembe Lagoon</rdfs:label>
    </owl:NamedIndividual>
    


    <!-- http://purl.obolibrary.org/obo/GAZ_00260965 -->

    <owl:NamedIndividual rdf:about="http://purl.obolibrary.org/obo/GAZ_00260965">
        <obo:RO_0001025 rdf:resource="http://purl.obolibrary.org/obo/GAZ_00058782"/>
        <obo:IAO_0000115>A lake on the Luapula Floodplain.</obo:IAO_0000115>
        <oboInOwl:hasOBONamespace>GAZ</oboInOwl:hasOBONamespace>
        <oboInOwl:id>GAZ:00260965</oboInOwl:id>
        <rdfs:label>Lake Kuswa</rdfs:label>
    </owl:NamedIndividual>
    


    <!-- http://purl.obolibrary.org/obo/GAZ_00260966 -->

    <owl:NamedIndividual rdf:about="http://purl.obolibrary.org/obo/GAZ_00260966">
        <obo:RO_0001025 rdf:resource="http://purl.obolibrary.org/obo/GAZ_00058782"/>
        <obo:IAO_0000115>A lake on the Luapula Floodplain.</obo:IAO_0000115>
        <oboInOwl:hasOBONamespace>GAZ</oboInOwl:hasOBONamespace>
        <oboInOwl:id>GAZ:00260966</oboInOwl:id>
        <rdfs:label>Lake Kitshomponshi</rdfs:label>
    </owl:NamedIndividual>
    


    <!-- http://purl.obolibrary.org/obo/GAZ_00260967 -->

    <owl:NamedIndividual rdf:about="http://purl.obolibrary.org/obo/GAZ_00260967">
        <obo:RO_0001025 rdf:resource="http://purl.obolibrary.org/obo/GAZ_00058782"/>
        <obo:IAO_0000115>A lake on the Luapula Floodplain.</obo:IAO_0000115>
        <oboInOwl:hasOBONamespace>GAZ</oboInOwl:hasOBONamespace>
        <oboInOwl:id>GAZ:00260967</oboInOwl:id>
        <rdfs:label>Lake Kifukula</rdfs:label>
    </owl:NamedIndividual>
    


    <!-- http://purl.obolibrary.org/obo/GAZ_00260968 -->

    <owl:NamedIndividual rdf:about="http://purl.obolibrary.org/obo/GAZ_00260968">
        <obo:RO_0001025 rdf:resource="http://purl.obolibrary.org/obo/GAZ_00058782"/>
        <obo:IAO_0000115>A lake on the Luapula Floodplain.</obo:IAO_0000115>
        <oboInOwl:hasOBONamespace>GAZ</oboInOwl:hasOBONamespace>
        <oboInOwl:id>GAZ:00260968</oboInOwl:id>
        <rdfs:label>Lake Kainsa</rdfs:label>
    </owl:NamedIndividual>
    


    <!-- http://purl.obolibrary.org/obo/GAZ_00260969 -->

    <owl:NamedIndividual rdf:about="http://purl.obolibrary.org/obo/GAZ_00260969">
        <obo:RO_0001025 rdf:resource="http://purl.obolibrary.org/obo/GAZ_00058782"/>
        <obo:IAO_0000115>A lake on the Luapula Floodplain.</obo:IAO_0000115>
        <oboInOwl:hasOBONamespace>GAZ</oboInOwl:hasOBONamespace>
        <oboInOwl:id>GAZ:00260969</oboInOwl:id>
        <rdfs:label>Lake Kinseneka</rdfs:label>
    </owl:NamedIndividual>
    


    <!-- http://purl.obolibrary.org/obo/GAZ_00260970 -->

    <owl:NamedIndividual rdf:about="http://purl.obolibrary.org/obo/GAZ_00260970">
        <obo:RO_0001025 rdf:resource="http://purl.obolibrary.org/obo/GAZ_00041532"/>
        <obo:IAO_0000115>An island.</obo:IAO_0000115>
        <oboInOwl:hasOBONamespace>GAZ</oboInOwl:hasOBONamespace>
        <oboInOwl:id>GAZ:00260970</oboInOwl:id>
        <rdfs:label>Katima Island</rdfs:label>
    </owl:NamedIndividual>
    


    <!-- http://purl.obolibrary.org/obo/GAZ_00260971 -->

    <owl:NamedIndividual rdf:about="http://purl.obolibrary.org/obo/GAZ_00260971">
        <obo:RO_0001025 rdf:resource="http://purl.obolibrary.org/obo/GAZ_00009423"/>
        <obo:IAO_0000115>A lake.</obo:IAO_0000115>
        <oboInOwl:hasOBONamespace>GAZ</oboInOwl:hasOBONamespace>
        <oboInOwl:id>GAZ:00260971</oboInOwl:id>
        <rdfs:label>Lake Cheshi</rdfs:label>
    </owl:NamedIndividual>
    


    <!-- http://purl.obolibrary.org/obo/GAZ_00260973 -->

    <owl:NamedIndividual rdf:about="http://purl.obolibrary.org/obo/GAZ_00260973">
        <obo:RO_0001025 rdf:resource="http://purl.obolibrary.org/obo/GAZ_00009429"/>
        <obo:IAO_0000115>A montaine lake. It drains eastwards through a short swampy area, before descending swiftly to the Luangwa River.</obo:IAO_0000115>
        <oboInOwl:hasOBONamespace>GAZ</oboInOwl:hasOBONamespace>
        <oboInOwl:id>GAZ:00260973</oboInOwl:id>
        <rdfs:label>Lake Lusiwasi</rdfs:label>
    </owl:NamedIndividual>
    


    <!-- http://purl.obolibrary.org/obo/GAZ_00260974 -->

    <owl:NamedIndividual rdf:about="http://purl.obolibrary.org/obo/GAZ_00260974">
        <obo:IAO_0000115>A reservoir. Completed 1978.</obo:IAO_0000115>
        <oboInOwl:hasOBONamespace>GAZ</oboInOwl:hasOBONamespace>
        <oboInOwl:id>GAZ:00260974</oboInOwl:id>
        <rdfs:label>Lake Itezhi-Tezhi</rdfs:label>
    </owl:NamedIndividual>
    


    <!-- http://purl.obolibrary.org/obo/GAZ_00260975 -->

    <owl:NamedIndividual rdf:about="http://purl.obolibrary.org/obo/GAZ_00260975">
        <obo:RO_0001025 rdf:resource="http://purl.obolibrary.org/obo/GAZ_00076754"/>
        <obo:IAO_0000115>Lakes. Small permanent pools that mark depressions in former Zambezi River channels which were abandoned as the main flow moved progressively northwards, towards the Zambian bank.</obo:IAO_0000115>
        <oboInOwl:hasOBONamespace>GAZ</oboInOwl:hasOBONamespace>
        <oboInOwl:id>GAZ:00260975</oboInOwl:id>
        <rdfs:label>Mana Pools</rdfs:label>
    </owl:NamedIndividual>
    


    <!-- http://purl.obolibrary.org/obo/GAZ_00260980 -->

    <owl:NamedIndividual rdf:about="http://purl.obolibrary.org/obo/GAZ_00260980">
        <obo:RO_0001025 rdf:resource="http://purl.obolibrary.org/obo/GAZ_00260975"/>
        <obo:IAO_0000115>A lake.</obo:IAO_0000115>
        <oboInOwl:hasOBONamespace>GAZ</oboInOwl:hasOBONamespace>
        <oboInOwl:id>GAZ:00260980</oboInOwl:id>
        <rdfs:label>Long Pool</rdfs:label>
    </owl:NamedIndividual>
    


    <!-- http://purl.obolibrary.org/obo/GAZ_00260981 -->

    <owl:NamedIndividual rdf:about="http://purl.obolibrary.org/obo/GAZ_00260981">
        <obo:RO_0001025 rdf:resource="http://purl.obolibrary.org/obo/GAZ_00260975"/>
        <obo:IAO_0000115>A lake.</obo:IAO_0000115>
        <oboInOwl:hasOBONamespace>GAZ</oboInOwl:hasOBONamespace>
        <oboInOwl:id>GAZ:00260981</oboInOwl:id>
        <rdfs:label>Chine Pool</rdfs:label>
    </owl:NamedIndividual>
    


    <!-- http://purl.obolibrary.org/obo/GAZ_00260996 -->

    <owl:NamedIndividual rdf:about="http://purl.obolibrary.org/obo/GAZ_00260996">
        <obo:RO_0001025 rdf:resource="http://purl.obolibrary.org/obo/GAZ_00016178"/>
        <obo:IAO_0000115>A river.</obo:IAO_0000115>
        <oboInOwl:hasOBONamespace>GAZ</oboInOwl:hasOBONamespace>
        <oboInOwl:id>GAZ:00260996</oboInOwl:id>
        <rdfs:label>Sebungwe River</rdfs:label>
    </owl:NamedIndividual>
    


    <!-- http://purl.obolibrary.org/obo/GAZ_00260997 -->

    <owl:NamedIndividual rdf:about="http://purl.obolibrary.org/obo/GAZ_00260997">
        <obo:RO_0001025 rdf:resource="http://purl.obolibrary.org/obo/GAZ_00016178"/>
        <obo:IAO_0000115>A river.</obo:IAO_0000115>
        <oboInOwl:hasOBONamespace>GAZ</oboInOwl:hasOBONamespace>
        <oboInOwl:id>GAZ:00260997</oboInOwl:id>
        <rdfs:label>Sengwa River</rdfs:label>
    </owl:NamedIndividual>
    


    <!-- http://purl.obolibrary.org/obo/GAZ_00260998 -->

    <owl:NamedIndividual rdf:about="http://purl.obolibrary.org/obo/GAZ_00260998">
        <obo:RO_0001025 rdf:resource="http://purl.obolibrary.org/obo/GAZ_00016178"/>
        <obo:IAO_0000115>A river.</obo:IAO_0000115>
        <oboInOwl:hasOBONamespace>GAZ</oboInOwl:hasOBONamespace>
        <oboInOwl:id>GAZ:00260998</oboInOwl:id>
        <rdfs:label>Ume River</rdfs:label>
    </owl:NamedIndividual>
    


    <!-- http://purl.obolibrary.org/obo/GAZ_00260999 -->

    <owl:NamedIndividual rdf:about="http://purl.obolibrary.org/obo/GAZ_00260999">
        <obo:RO_0001025 rdf:resource="http://purl.obolibrary.org/obo/GAZ_00016178"/>
        <obo:IAO_0000115>A river.</obo:IAO_0000115>
        <oboInOwl:hasOBONamespace>GAZ</oboInOwl:hasOBONamespace>
        <oboInOwl:id>GAZ:00260999</oboInOwl:id>
        <rdfs:label>Sanyati River</rdfs:label>
    </owl:NamedIndividual>
    


    <!-- http://purl.obolibrary.org/obo/GAZ_00261000 -->

    <owl:NamedIndividual rdf:about="http://purl.obolibrary.org/obo/GAZ_00261000">
        <obo:RO_0001025 rdf:resource="http://purl.obolibrary.org/obo/GAZ_00016178"/>
        <obo:IAO_0000115>A river.</obo:IAO_0000115>
        <oboInOwl:hasOBONamespace>GAZ</oboInOwl:hasOBONamespace>
        <oboInOwl:id>GAZ:00261000</oboInOwl:id>
        <rdfs:label>Mwenda River</rdfs:label>
    </owl:NamedIndividual>
    


    <!-- http://purl.obolibrary.org/obo/GAZ_00261001 -->

    <owl:NamedIndividual rdf:about="http://purl.obolibrary.org/obo/GAZ_00261001">
        <obo:RO_0001025 rdf:resource="http://purl.obolibrary.org/obo/GAZ_00016178"/>
        <obo:IAO_0000115>A river.</obo:IAO_0000115>
        <oboInOwl:hasOBONamespace>GAZ</oboInOwl:hasOBONamespace>
        <oboInOwl:id>GAZ:00261001</oboInOwl:id>
        <rdfs:label>Zhimu River</rdfs:label>
    </owl:NamedIndividual>
    


    <!-- http://purl.obolibrary.org/obo/GAZ_00261002 -->

    <owl:NamedIndividual rdf:about="http://purl.obolibrary.org/obo/GAZ_00261002">
        <obo:RO_0001025 rdf:resource="http://purl.obolibrary.org/obo/GAZ_00016178"/>
        <obo:IAO_0000115>A river.</obo:IAO_0000115>
        <oboInOwl:hasOBONamespace>GAZ</oboInOwl:hasOBONamespace>
        <oboInOwl:id>GAZ:00261002</oboInOwl:id>
        <rdfs:label>Zongwe River</rdfs:label>
    </owl:NamedIndividual>
    


    <!-- http://purl.obolibrary.org/obo/GAZ_00261003 -->

    <owl:NamedIndividual rdf:about="http://purl.obolibrary.org/obo/GAZ_00261003">
        <obo:RO_0001025 rdf:resource="http://purl.obolibrary.org/obo/GAZ_00016178"/>
        <obo:IAO_0000115>A river.</obo:IAO_0000115>
        <oboInOwl:hasOBONamespace>GAZ</oboInOwl:hasOBONamespace>
        <oboInOwl:id>GAZ:00261003</oboInOwl:id>
        <rdfs:label>Nangombe River</rdfs:label>
    </owl:NamedIndividual>
    


    <!-- http://purl.obolibrary.org/obo/GAZ_00261004 -->

    <owl:NamedIndividual rdf:about="http://purl.obolibrary.org/obo/GAZ_00261004">
        <obo:RO_0001025 rdf:resource="http://purl.obolibrary.org/obo/GAZ_00016178"/>
        <obo:IAO_0000115>A river.</obo:IAO_0000115>
        <oboInOwl:hasOBONamespace>GAZ</oboInOwl:hasOBONamespace>
        <oboInOwl:id>GAZ:00261004</oboInOwl:id>
        <rdfs:label>Chezya River</rdfs:label>
    </owl:NamedIndividual>
    


    <!-- http://purl.obolibrary.org/obo/GAZ_00261005 -->

    <owl:NamedIndividual rdf:about="http://purl.obolibrary.org/obo/GAZ_00261005">
        <obo:RO_0001025 rdf:resource="http://purl.obolibrary.org/obo/GAZ_00016178"/>
        <obo:IAO_0000115>A river.</obo:IAO_0000115>
        <oboInOwl:hasOBONamespace>GAZ</oboInOwl:hasOBONamespace>
        <oboInOwl:id>GAZ:00261005</oboInOwl:id>
        <rdfs:label>Chibue River</rdfs:label>
    </owl:NamedIndividual>
    


    <!-- http://purl.obolibrary.org/obo/GAZ_00261006 -->

    <owl:NamedIndividual rdf:about="http://purl.obolibrary.org/obo/GAZ_00261006">
        <obo:RO_0001025 rdf:resource="http://purl.obolibrary.org/obo/GAZ_00016178"/>
        <obo:IAO_0000115>A river.</obo:IAO_0000115>
        <oboInOwl:hasOBONamespace>GAZ</oboInOwl:hasOBONamespace>
        <oboInOwl:id>GAZ:00261006</oboInOwl:id>
        <rdfs:label>Lufue River</rdfs:label>
    </owl:NamedIndividual>
    


    <!-- http://purl.obolibrary.org/obo/GAZ_00261009 -->

    <owl:NamedIndividual rdf:about="http://purl.obolibrary.org/obo/GAZ_00261009">
        <obo:IAO_0000115>A dam. Located at Chitungwiza.</obo:IAO_0000115>
        <oboInOwl:hasOBONamespace>GAZ</oboInOwl:hasOBONamespace>
        <oboInOwl:id>GAZ:00261009</oboInOwl:id>
        <rdfs:label>Prince Edward Dam</rdfs:label>
    </owl:NamedIndividual>
    


    <!-- http://purl.obolibrary.org/obo/GAZ_00261010 -->

    <owl:NamedIndividual rdf:about="http://purl.obolibrary.org/obo/GAZ_00261010">
        <obo:IAO_0000115>A man-made lake.</obo:IAO_0000115>
        <oboInOwl:hasOBONamespace>GAZ</oboInOwl:hasOBONamespace>
        <oboInOwl:id>GAZ:00261010</oboInOwl:id>
        <rdfs:label>Lake Robertson</rdfs:label>
    </owl:NamedIndividual>
    


    <!-- http://purl.obolibrary.org/obo/GAZ_00261011 -->

    <owl:NamedIndividual rdf:about="http://purl.obolibrary.org/obo/GAZ_00261011">
        <obo:IAO_0000115>A dam.</obo:IAO_0000115>
        <oboInOwl:hasOBONamespace>GAZ</oboInOwl:hasOBONamespace>
        <oboInOwl:id>GAZ:00261011</oboInOwl:id>
        <rdfs:label>Dutchman&apos;s Pools Dam</rdfs:label>
    </owl:NamedIndividual>
    


    <!-- http://purl.obolibrary.org/obo/GAZ_00261012 -->

    <owl:NamedIndividual rdf:about="http://purl.obolibrary.org/obo/GAZ_00261012">
        <oboInOwl:hasOBONamespace>GAZ</oboInOwl:hasOBONamespace>
        <oboInOwl:id>GAZ:00261012</oboInOwl:id>
        <rdfs:label>Sebakwe Dam</rdfs:label>
    </owl:NamedIndividual>
    


    <!-- http://purl.obolibrary.org/obo/GAZ_00281450 -->

    <owl:NamedIndividual rdf:about="http://purl.obolibrary.org/obo/GAZ_00281450">
        <obo:RO_0001025 rdf:resource="http://purl.obolibrary.org/obo/GAZ_00009422"/>
        <obo:IAO_0000115>An archeological site.</obo:IAO_0000115>
        <oboInOwl:hasOBONamespace>GAZ</oboInOwl:hasOBONamespace>
        <oboInOwl:id>GAZ:00281450</oboInOwl:id>
        <rdfs:label>Ingombe Ilede</rdfs:label>
    </owl:NamedIndividual>
    


    <!-- http://purl.obolibrary.org/obo/GAZ_00281451 -->

    <owl:NamedIndividual rdf:about="http://purl.obolibrary.org/obo/GAZ_00281451">
        <obo:IAO_0000115>A single drop waterfall on the border of Zambia and Tanzania at the southeast end of Lake Tanganyika.</obo:IAO_0000115>
        <oboInOwl:hasOBONamespace>GAZ</oboInOwl:hasOBONamespace>
        <oboInOwl:id>GAZ:00281451</oboInOwl:id>
        <rdfs:label>Kalambo Falls</rdfs:label>
    </owl:NamedIndividual>
    


    <!-- http://purl.obolibrary.org/obo/GAZ_04000027 -->

    <owl:NamedIndividual rdf:about="http://purl.obolibrary.org/obo/GAZ_04000027">
        <rdf:type rdf:resource="http://purl.obolibrary.org/obo/ENVO_00000004"/>
        <obo:RO_0001025 rdf:resource="http://purl.obolibrary.org/obo/GAZ_00009420"/>
        <obo:IAO_0000115>A district of Lusaka Province.</obo:IAO_0000115>
        <oboInOwl:hasOBONamespace>GAZ</oboInOwl:hasOBONamespace>
        <oboInOwl:id>GAZ:04000027</oboInOwl:id>
        <rdfs:label>Lusaka District</rdfs:label>
    </owl:NamedIndividual>
    


    <!-- http://purl.obolibrary.org/obo/GAZ_04000028 -->

    <owl:NamedIndividual rdf:about="http://purl.obolibrary.org/obo/GAZ_04000028">
        <rdf:type rdf:resource="http://purl.obolibrary.org/obo/ENVO_00000004"/>
        <obo:RO_0001025 rdf:resource="http://purl.obolibrary.org/obo/GAZ_00009430"/>
        <obo:IAO_0000115>A district of Western Province.</obo:IAO_0000115>
        <oboInOwl:hasOBONamespace>GAZ</oboInOwl:hasOBONamespace>
        <oboInOwl:id>GAZ:04000028</oboInOwl:id>
        <rdfs:label>Mongu District</rdfs:label>
    </owl:NamedIndividual>
    


    <!-- 
    ///////////////////////////////////////////////////////////////////////////////////////
    //
    // Annotations
    //
    ///////////////////////////////////////////////////////////////////////////////////////
     -->

    <rdf:Description rdf:about="http://purl.obolibrary.org/obo/GAZ_00009419">
        <oboInOwl:hasOBONamespace>GAZ</oboInOwl:hasOBONamespace>
        <oboInOwl:id>GAZ:00009419</oboInOwl:id>
        <rdfs:label>Province (Zambia)</rdfs:label>
    </rdf:Description>
    <rdf:Description rdf:about="http://purl.obolibrary.org/obo/GAZ_00009420">
        <oboInOwl:id>GAZ:00009420</oboInOwl:id>
        <obo:IAO_0000115>One of Zambia&apos;s nine provinces. The provincial capital is Lusaka, which is also the national capital.</obo:IAO_0000115>
        <rdfs:label>Lusaka Province</rdfs:label>
        <oboInOwl:hasOBONamespace>GAZ</oboInOwl:hasOBONamespace>
    </rdf:Description>
    <rdf:Description rdf:about="http://purl.obolibrary.org/obo/GAZ_00009421">
        <obo:IAO_0000115>One of Zambia&apos;s nine provinces. The provincial capital is Chipata.</obo:IAO_0000115>
        <rdfs:label>Eastern Province</rdfs:label>
        <oboInOwl:id>GAZ:00009421</oboInOwl:id>
        <oboInOwl:hasOBONamespace>GAZ</oboInOwl:hasOBONamespace>
    </rdf:Description>
    <rdf:Description rdf:about="http://purl.obolibrary.org/obo/GAZ_00009422">
        <oboInOwl:id>GAZ:00009422</oboInOwl:id>
        <obo:IAO_0000115>One of Zambia&apos;s nine provinces. The Zambezi River is the province&apos;s southern border, and Lake Kariba, formed by the Kariba Dam, lies along the province&apos;s south-eastern edge. The eastern border is the Kariba Gorge and Zambezi, and the north-east border is the Kafue River and its gorge, dividing it from Lusaka Province. The Kafue Flats lie mostly within the province&apos;s northern border with Central Province. In the north west lies part of the famous Kafue National Park, the largest in Zambia, and the lake formed by the Itezhi-Tezhi Dam. The south-western border with Western Province runs through the teak forests around Mulobezi.</obo:IAO_0000115>
        <rdfs:label>Southern Province</rdfs:label>
        <oboInOwl:hasOBONamespace>GAZ</oboInOwl:hasOBONamespace>
    </rdf:Description>
    <rdf:Description rdf:about="http://purl.obolibrary.org/obo/GAZ_00009423">
        <rdfs:label>Northern Province</rdfs:label>
        <oboInOwl:id>GAZ:00009423</oboInOwl:id>
        <obo:IAO_0000115>One of Zambia&apos;s nine provinces. It covers approximately one fifth of Zambia in land area. The provincial capital is Kasama.</obo:IAO_0000115>
        <oboInOwl:hasOBONamespace>GAZ</oboInOwl:hasOBONamespace>
    </rdf:Description>
    <rdf:Description rdf:about="http://purl.obolibrary.org/obo/GAZ_00009425">
        <oboInOwl:id>GAZ:00009425</oboInOwl:id>
        <rdfs:label>Copperbelt Province</rdfs:label>
        <oboInOwl:hasOBONamespace>GAZ</oboInOwl:hasOBONamespace>
        <obo:IAO_0000115>A province of Zambia covers the mineral-rich Copperbelt. The province adjoins Katanga province of the Democratic Republic of the Congo, which is similarly mineral-rich.</obo:IAO_0000115>
    </rdf:Description>
    <rdf:Description rdf:about="http://purl.obolibrary.org/obo/GAZ_00009427">
        <oboInOwl:id>GAZ:00009427</oboInOwl:id>
        <obo:IAO_0000115>One of Zambia&apos;s nine provinces, and is located in the north of the country. The provincial capital is Mansa. It extends along the northern and eastern banks of the river from Lake Bangweulu to Lake Mweru, including waters and islands of those lakes.</obo:IAO_0000115>
        <oboInOwl:hasOBONamespace>GAZ</oboInOwl:hasOBONamespace>
        <rdfs:label>Luapula Province</rdfs:label>
    </rdf:Description>
    <rdf:Description rdf:about="http://purl.obolibrary.org/obo/GAZ_00009428">
        <oboInOwl:hasOBONamespace>GAZ</oboInOwl:hasOBONamespace>
        <oboInOwl:id>GAZ:00009428</oboInOwl:id>
        <rdfs:label>North-Western Province</rdfs:label>
        <obo:IAO_0000115>One of Zambia&apos;s nine provinces.</obo:IAO_0000115>
    </rdf:Description>
    <rdf:Description rdf:about="http://purl.obolibrary.org/obo/GAZ_00009429">
        <oboInOwl:hasOBONamespace>GAZ</oboInOwl:hasOBONamespace>
        <oboInOwl:id>GAZ:00009429</oboInOwl:id>
        <rdfs:label>Central Province</rdfs:label>
        <obo:IAO_0000115>One of Zambia&apos;s nine provinces. The provincial capital is Kabwe.</obo:IAO_0000115>
    </rdf:Description>
    <rdf:Description rdf:about="http://purl.obolibrary.org/obo/GAZ_00009430">
        <rdfs:label>Western Province</rdfs:label>
        <oboInOwl:id>GAZ:00009430</oboInOwl:id>
        <oboInOwl:hasOBONamespace>GAZ</oboInOwl:hasOBONamespace>
        <obo:IAO_0000115>One of Zambia&apos;s nine provinces.</obo:IAO_0000115>
    </rdf:Description>
    <rdf:Description rdf:about="http://purl.obolibrary.org/obo/GAZ_00010009">
        <oboInOwl:hasOBONamespace>GAZ</oboInOwl:hasOBONamespace>
        <rdfs:label>Lusaka</rdfs:label>
        <obo:IAO_0000115>A city that is the capital and largest city of Zambia. It is located in the southern part of the central plateau of the country, at an elevation of 1300 m.</obo:IAO_0000115>
        <oboInOwl:id>GAZ:00010009</oboInOwl:id>
    </rdf:Description>
    <rdf:Description rdf:about="http://purl.obolibrary.org/obo/GAZ_00010010">
        <oboInOwl:hasOBONamespace>GAZ</oboInOwl:hasOBONamespace>
        <obo:IAO_0000115>A small town and administrative district in the Western Province of Zambia, on the plains west of the Zambezi River and the Barotse Floodplain, about 70 km from the border with Angola.</obo:IAO_0000115>
        <oboInOwl:id>GAZ:00010010</oboInOwl:id>
        <rdfs:label>populated place, Zambia</rdfs:label>
    </rdf:Description>
    <rdf:Description rdf:about="http://purl.obolibrary.org/obo/GAZ_00010011">
        <oboInOwl:id>GAZ:00010011</oboInOwl:id>
        <rdfs:label>Mongu</rdfs:label>
        <obo:IAO_0000115>The capital of Western Province in Zambia.</obo:IAO_0000115>
        <oboInOwl:hasOBONamespace>GAZ</oboInOwl:hasOBONamespace>
    </rdf:Description>
    <rdf:Description rdf:about="http://purl.obolibrary.org/obo/GAZ_00052622">
        <oboInOwl:id>GAZ:00052622</oboInOwl:id>
        <rdfs:label>Solwezi</rdfs:label>
        <oboInOwl:hasOBONamespace>GAZ</oboInOwl:hasOBONamespace>
        <obo:IAO_0000115>A populated place. A town that is the capital of the North Western Province of Zambia.</obo:IAO_0000115>
    </rdf:Description>
    <rdf:Description rdf:about="http://purl.obolibrary.org/obo/GAZ_00052623">
        <obo:IAO_0000115>A populated place. A town in the Northern Province of Zambia, lying at the junction of the Great North Road to Kasama and Mbala and the Tanzam Highway to Dar es Salaam, Tanzania.</obo:IAO_0000115>
        <oboInOwl:id>GAZ:00052623</oboInOwl:id>
        <oboInOwl:hasOBONamespace>GAZ</oboInOwl:hasOBONamespace>
        <rdfs:label>Mpika</rdfs:label>
    </rdf:Description>
    <rdf:Description rdf:about="http://purl.obolibrary.org/obo/GAZ_00052624">
        <rdfs:label>Mbala</rdfs:label>
        <oboInOwl:hasOBONamespace>GAZ</oboInOwl:hasOBONamespace>
        <obo:IAO_0000115>A populated place. A town occupying a strategic location close to the border with Tanzania and controlling the southern approaches to Lake Tanganyika, 40 km by road to the north-east, where the port of Mpulungu is located.</obo:IAO_0000115>
        <oboInOwl:id>GAZ:00052624</oboInOwl:id>
    </rdf:Description>
    <rdf:Description rdf:about="http://purl.obolibrary.org/obo/GAZ_00052625">
        <rdfs:label>Simonga</rdfs:label>
        <oboInOwl:hasOBONamespace>GAZ</oboInOwl:hasOBONamespace>
        <oboInOwl:id>GAZ:00052625</oboInOwl:id>
        <obo:IAO_0000115>A populated place.</obo:IAO_0000115>
    </rdf:Description>
    <rdf:Description rdf:about="http://purl.obolibrary.org/obo/GAZ_00052628">
        <oboInOwl:hasOBONamespace>GAZ</oboInOwl:hasOBONamespace>
        <rdfs:label>Mansa</rdfs:label>
        <oboInOwl:id>GAZ:00052628</oboInOwl:id>
        <obo:IAO_0000115>A populated place. A town that is the capital of the Luapula Province of Zambia, and headquarters of Mansa district. It takes its name from the local Chief Mansa and the small Mansa River which flows west to the Luapula River.</obo:IAO_0000115>
    </rdf:Description>
    <rdf:Description rdf:about="http://purl.obolibrary.org/obo/GAZ_00052631">
        <oboInOwl:id>GAZ:00052631</oboInOwl:id>
        <oboInOwl:hasOBONamespace>GAZ</oboInOwl:hasOBONamespace>
        <obo:IAO_0000115>A populated place.</obo:IAO_0000115>
        <rdfs:label>Kasyasya</rdfs:label>
    </rdf:Description>
    <rdf:Description rdf:about="http://purl.obolibrary.org/obo/GAZ_00052641">
        <oboInOwl:hasOBONamespace>GAZ</oboInOwl:hasOBONamespace>
        <oboInOwl:id>GAZ:00052641</oboInOwl:id>
        <obo:IAO_0000115>A populated place. A town in the Western Province of Zambia, on the eastern bank of the Zambezi River, at the southern end of its Barotse Floodplain.</obo:IAO_0000115>
        <rdfs:label>Senanga</rdfs:label>
    </rdf:Description>
    <rdf:Description rdf:about="http://purl.obolibrary.org/obo/GAZ_00052643">
        <oboInOwl:hasOBONamespace>GAZ</oboInOwl:hasOBONamespace>
        <oboInOwl:id>GAZ:00052643</oboInOwl:id>
        <rdfs:label>Sekute</rdfs:label>
        <obo:IAO_0000115>A populated place.</obo:IAO_0000115>
    </rdf:Description>
    <rdf:Description rdf:about="http://purl.obolibrary.org/obo/GAZ_00052644">
        <oboInOwl:id>GAZ:00052644</oboInOwl:id>
        <rdfs:label>Ndola</rdfs:label>
        <oboInOwl:hasOBONamespace>GAZ</oboInOwl:hasOBONamespace>
        <obo:IAO_0000115>A city that is the industrial, commercial, administrative and distribution hub of the Copperbelt, Zambia&apos;s copper-mining region, and capital of Copperbelt Province.</obo:IAO_0000115>
    </rdf:Description>
    <rdf:Description rdf:about="http://purl.obolibrary.org/obo/GAZ_00052645">
        <oboInOwl:id>GAZ:00052645</oboInOwl:id>
        <rdfs:label>Macha</rdfs:label>
        <obo:IAO_0000115>A populated place.</obo:IAO_0000115>
        <oboInOwl:hasOBONamespace>GAZ</oboInOwl:hasOBONamespace>
    </rdf:Description>
    <rdf:Description rdf:about="http://purl.obolibrary.org/obo/GAZ_00052647">
        <oboInOwl:id>GAZ:00052647</oboInOwl:id>
        <obo:IAO_0000115>A city and present capital of the Southern Province of Zambia.</obo:IAO_0000115>
        <rdfs:label>Livingstone</rdfs:label>
        <oboInOwl:hasOBONamespace>GAZ</oboInOwl:hasOBONamespace>
    </rdf:Description>
    <rdf:Description rdf:about="http://purl.obolibrary.org/obo/GAZ_00052651">
        <oboInOwl:id>GAZ:00052651</oboInOwl:id>
        <obo:IAO_0000115>A small town and administrative district in the Western Province of Zambia, on the plains west of the Zambezi River and the Barotse Floodplain, about 70 km from the border with Angola.</obo:IAO_0000115>
        <oboInOwl:hasOBONamespace>GAZ</oboInOwl:hasOBONamespace>
        <rdfs:label>Kalabo</rdfs:label>
    </rdf:Description>
    <rdf:Description rdf:about="http://purl.obolibrary.org/obo/GAZ_00052654">
        <oboInOwl:hasOBONamespace>GAZ</oboInOwl:hasOBONamespace>
        <oboInOwl:id>GAZ:00052654</oboInOwl:id>
        <obo:IAO_0000115>A populated place. A town that is the capital of the Northern Province of Zambia, situated on the central-southern African plateau at an elevation of about 1400 m.</obo:IAO_0000115>
        <rdfs:label>Kasama</rdfs:label>
    </rdf:Description>
    <rdf:Description rdf:about="http://purl.obolibrary.org/obo/GAZ_00052655">
        <rdfs:label>Kataba</rdfs:label>
        <obo:IAO_0000115>A populated place. A town located in the Western Province of Zambia.</obo:IAO_0000115>
        <oboInOwl:hasOBONamespace>GAZ</oboInOwl:hasOBONamespace>
        <oboInOwl:id>GAZ:00052655</oboInOwl:id>
    </rdf:Description>
    <rdf:Description rdf:about="http://purl.obolibrary.org/obo/GAZ_00052656">
        <obo:IAO_0000115>A populated place. A city in Zambia in the centre of the Copperbelt, Zambia&apos;s copper-mining region.</obo:IAO_0000115>
        <oboInOwl:id>GAZ:00052656</oboInOwl:id>
        <rdfs:label>Kitwe</rdfs:label>
        <oboInOwl:hasOBONamespace>GAZ</oboInOwl:hasOBONamespace>
    </rdf:Description>
    <rdf:Description rdf:about="http://purl.obolibrary.org/obo/GAZ_00052661">
        <obo:IAO_0000115>A populated place. A town in the Northern Province of Zambia, at the southern tip of Lake Tanganyika. It is landlocked Zambia&apos;s only port.</obo:IAO_0000115>
        <oboInOwl:id>GAZ:00052661</oboInOwl:id>
        <oboInOwl:hasOBONamespace>GAZ</oboInOwl:hasOBONamespace>
        <rdfs:label>Mpulungu</rdfs:label>
    </rdf:Description>
</rdf:RDF>



<!-- Generated by the OWL API (version 4.5.6) https://github.com/owlcs/owlapi -->

